@prefix bibo: <http://purl.org/ontology/bibo/> .
@prefix dct: <http://purl.org/dc/terms/> .
@prefix dpv-owl: <https://w3id.org/dpv/owl#> .
@prefix foaf: <http://xmlns.com/foaf/0.1/> .
@prefix loc-owl: <https://w3id.org/dpv/loc/owl#> .
@prefix owl: <http://www.w3.org/2002/07/owl#> .
@prefix profile: <http://www.w3.org/ns/dx/prof/> .
@prefix rdf: <http://www.w3.org/1999/02/22-rdf-syntax-ns#> .
@prefix rdfs: <http://www.w3.org/2000/01/rdf-schema#> .
@prefix role: <http://www.w3.org/ns/dx/prof/role/> .
@prefix schema: <https://schema.org/> .
@prefix skos: <http://www.w3.org/2004/02/skos/core#> .
@prefix sw: <http://www.w3.org/2003/06/sw-vocab-status/ns#> .
@prefix time: <http://www.w3.org/2006/time#> .
@prefix vann: <http://purl.org/vocab/vann/> .
@prefix xsd: <http://www.w3.org/2001/XMLSchema#> .

loc-owl:EEA a rdfs:Class,
        owl:Class,
        dpv-owl:SupraNationalUnion ;
    dct:contributor "Harshvardhan J. Pandit" ;
    dct:created "2022-03-30"^^xsd:date ;
    rdfs:isDefinedBy loc-owl: ;
    rdfs:subClassOf dpv-owl:SupraNationalUnion ;
    sw:term_status "accepted"@en ;
    skos:definition "Concept representing the latest membership of European Economic Area (EEA)"@en ;
    skos:prefLabel "European Economic Area (EEA)"@en .

loc-owl:EEA30 a rdfs:Class,
        owl:Class,
        dpv-owl:SupraNationalUnion ;
    dct:contributor "Harshvardhan J. Pandit" ;
    dct:created "2022-03-30"^^xsd:date ;
    dct:modified "2024-04-15"^^xsd:date ;
    dct:temporal [ a time:ProperInterval ;
            time:hasBeginning [ time:inXSDDate "2020-02-01"^^xsd:date ] ] ;
    rdfs:isDefinedBy loc-owl: ;
    rdfs:subClassOf loc-owl:EEA ;
    sw:term_status "accepted"@en ;
    skos:definition "Concept represent current EEA with 30 Member States that became active from 2020 with exit of UK from EEA31 after Brexit"@en ;
    skos:prefLabel "EEA 30 Member States"@en ;
    skos:scopeNote "European Economic Area (EEA-31) with 30 Member States post Brexit"@en .

loc-owl:EEA31 a rdfs:Class,
        owl:Class,
        dpv-owl:SupraNationalUnion ;
    dct:contributor "Harshvardhan J. Pandit" ;
    dct:created "2022-03-30"^^xsd:date ;
    dct:modified "2024-04-15"^^xsd:date ;
    dct:temporal [ a time:ProperInterval ;
            time:hasBeginning [ time:inXSDDate "2014-04-12"^^xsd:date ] ;
            time:hasEnd [ time:inXSDDate "2020-01-31"^^xsd:date ] ] ;
    rdfs:isDefinedBy loc-owl: ;
    rdfs:subClassOf loc-owl:EEA ;
    sw:term_status "accepted"@en ;
    skos:definition "Concept representing previous EEA with 31 Member States that was active from 2014 and concluded with the exit of UK in 2022 after Brexit"@en ;
    skos:prefLabel "EEA 31 Member States"@en ;
    skos:scopeNote "European Economic Area (EEA-31) with 30 Member States pre Brexit"@en .

loc-owl:EU a rdfs:Class,
        owl:Class,
        dpv-owl:SupraNationalUnion ;
    dct:contributor "Harshvardhan J. Pandit" ;
    dct:created "2022-03-30"^^xsd:date ;
    rdfs:isDefinedBy loc-owl: ;
    rdfs:subClassOf dpv-owl:SupraNationalUnion ;
    sw:term_status "accepted"@en ;
    skos:definition "Concept representing the latest membership of European Union (EU)"@en ;
    skos:prefLabel "European Union (EU)"@en .

loc-owl:EU27 a rdfs:Class,
        owl:Class,
        dpv-owl:SupraNationalUnion ;
    dct:contributor "Harshvardhan J. Pandit" ;
    dct:created "2022-03-30"^^xsd:date ;
    dct:temporal [ a time:ProperInterval ;
            time:hasBeginning [ time:inXSDDate "2020-02-01"^^xsd:date ] ] ;
    rdfs:isDefinedBy loc-owl: ;
    rdfs:subClassOf loc-owl:EU ;
    sw:term_status "accepted"@en ;
    skos:definition "Concept representing current EU with 27 Member States that became active from 2020 with exit of UK from EEA31 after Brexit"@en ;
    skos:prefLabel "EU 27 Member States"@en ;
    skos:scopeNote "European Union (EU-27) with 27 Member States post Brexit. Note that EU27 is also applicable to the 27 Member States in the EU from 2007 to 2013, which is not represented in the LOC extension. If this concept should exist, please submit an issue or proposal"@en .

loc-owl:EU28 a rdfs:Class,
        owl:Class,
        dpv-owl:SupraNationalUnion ;
    dct:contributor "Harshvardhan J. Pandit" ;
    dct:created "2022-03-30"^^xsd:date ;
    dct:temporal [ a time:ProperInterval ;
            time:hasBeginning [ time:inXSDDate "2013-07-01"^^xsd:date ] ;
            time:hasEnd [ time:inXSDDate "2020-01-31"^^xsd:date ] ] ;
    rdfs:isDefinedBy loc-owl: ;
    rdfs:subClassOf loc-owl:EU ;
    sw:term_status "accepted"@en ;
    skos:definition "Concept representing previous EEA with 31 Member States that was active from 2014 and concluded with the exit of UK in 2022 after Brexit"@en ;
    skos:prefLabel "EU 28 Member States"@en ;
    skos:scopeNote "European Union (EU-28) with 28 Member States pre Brexit"@en .

loc-owl:serialisation-html a profile:ResourceDescriptor ;
    dct:conformsTo <https://www.w3.org/TR/html/> ;
    dct:format <https://www.iana.org/assignments/media-types/text/html> ;
    dct:title "Location Concepts - HTML serialiation" ;
    profile:hasArtifact <https://w3id.org/dpv/loc/loc-owl.html> ;
    profile:hasRole role:specification .

loc-owl:serialisation-jsonld a profile:ResourceDescriptor ;
    dct:conformsTo <https://www.w3.org/TR/json-ld11/> ;
    dct:format <https://www.iana.org/assignments/media-types/application/ld+json> ;
    dct:title "Location Concepts - JSON-LD serialiation" ;
    profile:hasArtifact <https://w3id.org/dpv/loc/loc-owl.jsonld> ;
    profile:hasRole role:vocabulary .

loc-owl:serialisation-n3 a profile:ResourceDescriptor ;
    dct:conformsTo <https://www.w3.org/TeamSubmission/n3/> ;
    dct:format <https://www.iana.org/assignments/media-types/text/n3> ;
    dct:title "Location Concepts - N3 serialiation" ;
    profile:hasArtifact <https://w3id.org/dpv/loc/loc-owl.n3> ;
    profile:hasRole role:vocabulary .

loc-owl:serialisation-rdf a profile:ResourceDescriptor ;
    dct:conformsTo rdf: ;
    dct:format <https://www.iana.org/assignments/media-types/application/rdf+xml> ;
    dct:title "Location Concepts - RDF/XML serialiation" ;
    profile:hasArtifact <https://w3id.org/dpv/loc/loc-owl.rdf> ;
    profile:hasRole role:vocabulary .

loc-owl:serialisation-ttl a profile:ResourceDescriptor ;
    dct:conformsTo <https://www.w3.org/TR/turtle/> ;
    dct:format <https://www.iana.org/assignments/media-types/text/turtle> ;
    dct:title "Location Concepts - Turtle serialiation" ;
    profile:hasArtifact <https://w3id.org/dpv/loc/loc-owl.ttl> ;
    profile:hasRole role:vocabulary .

<https://w3id.org/dpv/examples> a profile:ResourceDescriptor ;
    dct:conformsTo <https://www.w3.org/TR/html/> ;
    dct:format <https://www.iana.org/assignments/media-types/text/html> ;
    dct:title "Examples for Data Privacy Vocabulary" ;
    profile:hasArtifact <https://w3id.org/dpv/examples> ;
    profile:hasRole role:guidance .

<https://w3id.org/dpv/guides> a profile:ResourceDescriptor ;
    dct:conformsTo <https://www.w3.org/TR/html/> ;
    dct:format <https://www.iana.org/assignments/media-types/text/html> ;
    dct:title "Guides for Data Privacy Vocabulary" ;
    profile:hasArtifact <https://w3id.org/dpv/guides> ;
    profile:hasRole role:guidance .

<https://w3id.org/dpv/primer> a profile:ResourceDescriptor ;
    dct:conformsTo <https://www.w3.org/TR/html/> ;
    dct:format <https://www.iana.org/assignments/media-types/text/html> ;
    dct:title "Primer for Data Privacy Vocabulary" ;
    profile:hasArtifact <https://w3id.org/dpv/primer> ;
    profile:hasRole role:guidance .

loc-owl: a owl:Ontology,
        profile:Profile ;
    dct:bibliographicCitation "Data Privacy Vocabulary (DPV) -- Version 2. Harshvardhan J. Pandit, Beatriz Esteves, Georg P. Krog, Paul Ryan, Delaram Golpayegani, Julian Flake https://doi.org/10.48550/arXiv.2404.13426" ;
    dct:conformsTo <http://www.w3.org/2002/07/owl>,
        "http://www.w3.org/2000/01/rdf-schema",
        "http://www.w3.org/2004/02/skos/core" ;
    dct:contributor "Harshvardhan J. Pandit" ;
    dct:created "2022-04-02"@en ;
    dct:creator "Harshvardhan J. Pandit"@en ;
    dct:description "Extension to the Data Privacy Vocabulary (DPV) providing concepts for representing (geo-political) locations and memberships"@en ;
    dct:hasVersion loc-owl: ;
    dct:identifier "https://w3id.org/dpv/loc" ;
    dct:issued "2022-04-02"@en ;
    dct:license <https://www.w3.org/copyright/document-license-2023/> ;
    dct:modified "2024-07-01"@en ;
    dct:publisher <https://www.w3.org/> ;
    dct:source <https://www.w3.org/groups/cg/dpvcg/> ;
    dct:title "Location Concepts"@en ;
    bibo:doi "10.5281/zenodo.12505841" ;
    bibo:status "http://purl.org/ontology/bibo/status/published" ;
    vann:preferredNamespacePrefix "loc" ;
    vann:preferredNamespaceUri "https://w3id.org/dpv/loc#" ;
    rdfs:Label "LOC"@en ;
    owl:versionIRI <https://w3id.org/dpv/2.0/loc/owl#> ;
    owl:versionInfo "2.0" ;
    profile:hasResource <https://w3id.org/dpv/examples>,
        <https://w3id.org/dpv/guides>,
        loc-owl:serialisation-html,
        loc-owl:serialisation-jsonld,
        loc-owl:serialisation-n3,
        loc-owl:serialisation-rdf,
        loc-owl:serialisation-ttl,
        <https://w3id.org/dpv/primer> ;
    profile:isProfileOf <http://www.w3.org/2002/07/owl>,
        loc-owl:,
        <https://w3id.org/dpv/owl> ;
    foaf:logo <https://w3id.org/dpv/media/logo.png> ;
    schema:version "2.0" .

