@prefix bibo: <http://purl.org/ontology/bibo/> .
@prefix dct: <http://purl.org/dc/terms/> .
@prefix dpv-owl: <https://w3id.org/dpv/owl#> .
@prefix foaf: <http://xmlns.com/foaf/0.1/> .
@prefix org: <http://www.w3.org/ns/org#> .
@prefix owl: <http://www.w3.org/2002/07/owl#> .
@prefix profile: <http://www.w3.org/ns/dx/prof/> .
@prefix rdf: <http://www.w3.org/1999/02/22-rdf-syntax-ns#> .
@prefix rdfs: <http://www.w3.org/2000/01/rdf-schema#> .
@prefix role: <http://www.w3.org/ns/dx/prof/role/> .
@prefix schema: <https://schema.org/> .
@prefix scoro: <http://purl.org/spar/scoro/> .
@prefix skos: <http://www.w3.org/2004/02/skos/core#> .
@prefix sw: <http://www.w3.org/2003/06/sw-vocab-status/ns#> .
@prefix tech-owl: <https://w3id.org/dpv/tech/owl#> .
@prefix vann: <http://purl.org/vocab/vann/> .
@prefix xsd: <http://www.w3.org/2001/XMLSchema#> .

tech-owl:Action a rdfs:Class,
        owl:Class ;
    dct:contributor _:person-delaram-golpayegani,
        _:person-harshvardhan-j-pandit ;
    dct:created "2024-12-01"^^xsd:date ;
    rdfs:isDefinedBy tech-owl: ;
    rdfs:subClassOf tech-owl:InputOutput ;
    sw:term_status "accepted"@en ;
    skos:definition "A process or activity, which could be physical or virtual"@en ;
    skos:prefLabel "Action"@en ;
    skos:scopeNote "Action is a concept referring to activities or tasks in the context of technologies producing or using them as inputs or outputs"@en .

tech-owl:AudioContent a rdfs:Class,
        owl:Class ;
    dct:contributor _:person-delaram-golpayegani,
        _:person-harshvardhan-j-pandit ;
    dct:created "2024-12-01"^^xsd:date ;
    rdfs:isDefinedBy tech-owl: ;
    rdfs:subClassOf tech-owl:Content ;
    sw:term_status "accepted"@en ;
    skos:definition "Content that is or has an audio component"@en ;
    skos:prefLabel "Audio Content"@en .

tech-owl:Content a rdfs:Class,
        owl:Class ;
    dct:contributor _:person-delaram-golpayegani,
        _:person-harshvardhan-j-pandit ;
    dct:created "2024-12-01"^^xsd:date ;
    rdfs:isDefinedBy tech-owl: ;
    rdfs:subClassOf dpv-owl:Data,
        tech-owl:InputOutput ;
    sw:term_status "accepted"@en ;
    skos:definition "Data or information in a particular form and structure"@en ;
    skos:prefLabel "Content"@en ;
    skos:scopeNote "Content is a concept referring to information used in the context of technologies producing or using them as inputs or outputs"@en .

tech-owl:Decision a rdfs:Class,
        owl:Class ;
    dct:contributor _:person-delaram-golpayegani,
        _:person-harshvardhan-j-pandit ;
    dct:created "2024-12-01"^^xsd:date ;
    rdfs:isDefinedBy tech-owl: ;
    rdfs:subClassOf tech-owl:InputOutput ;
    sw:term_status "accepted"@en ;
    skos:definition "A conclusion or determination of an action or choice in the context of technologies"@en ;
    skos:prefLabel "Decision"@en ;
    skos:scopeNote "Decision is a concept referring to activities or tasks in the context of technologies producing or using them as inputs or outputs"@en .

tech-owl:ImageContent a rdfs:Class,
        owl:Class ;
    dct:contributor _:person-delaram-golpayegani,
        _:person-harshvardhan-j-pandit ;
    dct:created "2024-12-01"^^xsd:date ;
    rdfs:isDefinedBy tech-owl: ;
    rdfs:subClassOf tech-owl:Content ;
    sw:term_status "accepted"@en ;
    skos:definition "Content that is or has an image component"@en ;
    skos:prefLabel "Image Content"@en .

tech-owl:Input a rdfs:Class,
        owl:Class ;
    dct:contributor _:person-delaram-golpayegani,
        _:person-harshvardhan-j-pandit ;
    dct:created "2024-12-01"^^xsd:date ;
    rdfs:isDefinedBy tech-owl: ;
    rdfs:subClassOf tech-owl:InputOutput ;
    sw:term_status "accepted"@en ;
    skos:definition "Input to a technology"@en ;
    skos:prefLabel "Input"@en .

tech-owl:InputAction a rdfs:Class,
        owl:Class ;
    dct:contributor _:person-delaram-golpayegani,
        _:person-harshvardhan-j-pandit ;
    dct:created "2024-12-01"^^xsd:date ;
    rdfs:isDefinedBy tech-owl: ;
    rdfs:subClassOf tech-owl:Action,
        tech-owl:Input ;
    sw:term_status "accepted"@en ;
    skos:definition "Action provided as an input to a technology"@en ;
    skos:prefLabel "Input Action"@en ;
    skos:scopeNote "Action can mean a physical action, such as the movements involved in robotics"@en .

tech-owl:InputData a rdfs:Class,
        owl:Class ;
    dct:contributor _:person-delaram-golpayegani,
        _:person-harshvardhan-j-pandit ;
    dct:created "2024-12-01"^^xsd:date ;
    rdfs:isDefinedBy tech-owl: ;
    rdfs:subClassOf dpv-owl:Data,
        tech-owl:Input ;
    sw:term_status "accepted"@en ;
    skos:definition "Data that is provided an input to a technology"@en ;
    skos:prefLabel "Input Data"@en .

tech-owl:Output a rdfs:Class,
        owl:Class ;
    dct:contributor _:person-delaram-golpayegani,
        _:person-harshvardhan-j-pandit ;
    dct:created "2024-12-01"^^xsd:date ;
    rdfs:isDefinedBy tech-owl: ;
    rdfs:subClassOf tech-owl:InputOutput ;
    sw:term_status "accepted"@en ;
    skos:definition "Output from a technology"@en ;
    skos:prefLabel "Output"@en .

tech-owl:OutputAction a rdfs:Class,
        owl:Class ;
    dct:contributor _:person-delaram-golpayegani,
        _:person-harshvardhan-j-pandit ;
    dct:created "2024-12-01"^^xsd:date ;
    rdfs:isDefinedBy tech-owl: ;
    rdfs:subClassOf tech-owl:Action,
        tech-owl:Output ;
    sw:term_status "accepted"@en ;
    skos:definition "Action produced as an output from a technology"@en ;
    skos:prefLabel "Output Action"@en ;
    skos:scopeNote "Action can mean a physical action, such as the movements involved in robotics"@en .

tech-owl:OutputData a rdfs:Class,
        owl:Class ;
    dct:contributor _:person-delaram-golpayegani,
        _:person-harshvardhan-j-pandit ;
    dct:created "2024-12-01"^^xsd:date ;
    rdfs:isDefinedBy tech-owl: ;
    rdfs:subClassOf dpv-owl:Data,
        tech-owl:Output ;
    sw:term_status "accepted"@en ;
    skos:definition "Data that is produced as an output from a technology"@en ;
    skos:prefLabel "Output Data"@en .

tech-owl:Prediction a rdfs:Class,
        owl:Class ;
    dct:contributor _:person-delaram-golpayegani,
        _:person-harshvardhan-j-pandit ;
    dct:created "2024-12-01"^^xsd:date ;
    rdfs:isDefinedBy tech-owl: ;
    rdfs:subClassOf tech-owl:InputOutput ;
    sw:term_status "accepted"@en ;
    skos:definition "An inference or prediction of an action or data or decision in the context of technologies"@en ;
    skos:prefLabel "Prediction"@en ;
    skos:scopeNote "Prediction is a concept referring to activities or tasks in the context of technologies producing or using them as inputs or outputs"@en .

tech-owl:Recommendation a rdfs:Class,
        owl:Class ;
    dct:contributor _:person-delaram-golpayegani,
        _:person-harshvardhan-j-pandit ;
    dct:created "2024-12-01"^^xsd:date ;
    rdfs:isDefinedBy tech-owl: ;
    rdfs:subClassOf tech-owl:InputOutput ;
    sw:term_status "accepted"@en ;
    skos:definition "A recommendation or suggestion of an action or decision or choice in the context of technologies"@en ;
    skos:prefLabel "Recommendation"@en ;
    skos:scopeNote "Recommendation is a concept referring to activities or tasks in the context of technologies producing or using them as inputs or outputs"@en .

tech-owl:TextualContent a rdfs:Class,
        owl:Class ;
    dct:contributor _:person-delaram-golpayegani,
        _:person-harshvardhan-j-pandit ;
    dct:created "2024-12-01"^^xsd:date ;
    rdfs:isDefinedBy tech-owl: ;
    rdfs:subClassOf tech-owl:Content ;
    sw:term_status "accepted"@en ;
    skos:definition "Content that is or has a textual component"@en ;
    skos:prefLabel "Textual Content"@en .

tech-owl:VideoContent a rdfs:Class,
        owl:Class ;
    dct:contributor _:person-delaram-golpayegani,
        _:person-harshvardhan-j-pandit ;
    dct:created "2024-12-01"^^xsd:date ;
    rdfs:isDefinedBy tech-owl: ;
    rdfs:subClassOf tech-owl:Content ;
    sw:term_status "accepted"@en ;
    skos:definition "Content that is or has a video component"@en ;
    skos:prefLabel "Video Content"@en .

tech-owl:serialisation-html a profile:ResourceDescriptor ;
    dct:conformsTo <https://www.w3.org/TR/html/> ;
    dct:format <https://www.iana.org/assignments/media-types/text/html> ;
    dct:title "Technology Concepts - HTML serialisation" ;
    profile:hasArtifact <https://w3id.org/dpv/tech/tech-owl.html> ;
    profile:hasRole role:specification .

tech-owl:serialisation-jsonld a profile:ResourceDescriptor ;
    dct:conformsTo <https://www.w3.org/TR/json-ld11/> ;
    dct:format <https://www.iana.org/assignments/media-types/application/ld+json> ;
    dct:title "Technology Concepts - JSON-LD serialisation" ;
    profile:hasArtifact <https://w3id.org/dpv/tech/tech-owl.jsonld> ;
    profile:hasRole role:vocabulary .

tech-owl:serialisation-n3 a profile:ResourceDescriptor ;
    dct:conformsTo <https://www.w3.org/TeamSubmission/n3/> ;
    dct:format <https://www.iana.org/assignments/media-types/text/n3> ;
    dct:title "Technology Concepts - N3 serialisation" ;
    profile:hasArtifact <https://w3id.org/dpv/tech/tech-owl.n3> ;
    profile:hasRole role:vocabulary .

tech-owl:serialisation-rdf a profile:ResourceDescriptor ;
    dct:conformsTo rdf: ;
    dct:format <https://www.iana.org/assignments/media-types/application/rdf+xml> ;
    dct:title "Technology Concepts - RDF/XML serialisation" ;
    profile:hasArtifact <https://w3id.org/dpv/tech/tech-owl.rdf> ;
    profile:hasRole role:vocabulary .

tech-owl:serialisation-ttl a profile:ResourceDescriptor ;
    dct:conformsTo <https://www.w3.org/TR/turtle/> ;
    dct:format <https://www.iana.org/assignments/media-types/text/turtle> ;
    dct:title "Technology Concepts - Turtle serialisation" ;
    profile:hasArtifact <https://w3id.org/dpv/tech/tech-owl.ttl> ;
    profile:hasRole role:vocabulary .

<https://w3id.org/dpv/examples> a profile:ResourceDescriptor ;
    dct:conformsTo <https://www.w3.org/TR/html/> ;
    dct:format <https://www.iana.org/assignments/media-types/text/html> ;
    dct:title "Examples" ;
    profile:hasArtifact <https://w3id.org/dpv/examples> ;
    profile:hasRole role:guidance .

<https://w3id.org/dpv/guides> a profile:ResourceDescriptor ;
    dct:conformsTo <https://www.w3.org/TR/html/> ;
    dct:format <https://www.iana.org/assignments/media-types/text/html> ;
    dct:title "Guides for Data Privacy Vocabulary" ;
    profile:hasArtifact <https://w3id.org/dpv/guides> ;
    profile:hasRole role:guidance .

<https://w3id.org/dpv/primer> a profile:ResourceDescriptor ;
    dct:conformsTo <https://www.w3.org/TR/html/> ;
    dct:format <https://www.iana.org/assignments/media-types/text/html> ;
    dct:title "Primer for Data Privacy Vocabulary" ;
    profile:hasArtifact <https://w3id.org/dpv/primer> ;
    profile:hasRole role:guidance .

tech-owl: a owl:Ontology,
        profile:Profile ;
    dct:bibliographicCitation "Harshvardhan J. Pandit, Beatriz Esteves, Georg P. Krog, Paul Ryan, Delaram Golpayegani, Julian Flake (2025) Data Privacy Vocabulary (DPV) – Version 2.0. In: Demartini, G., et al. The Semantic Web – ISWC 2024. ISWC 2024. Lecture Notes in Computer Science, vol 15233. Springer, Cham. https://doi.org/10.1007/978-3-031-77847-6_10" ;
    dct:conformsTo <http://www.w3.org/2002/07/owl>,
        "http://www.w3.org/2000/01/rdf-schema",
        "http://www.w3.org/2004/02/skos/core" ;
    dct:contributor _:person-delaram-golpayegani,
        _:person-harshvardhan-j-pandit ;
    dct:created "2024-05-31"@en ;
    dct:creator _:person-delaram-golpayegani,
        [ a dct:Agent,
                foaf:Person ;
            org:memberOf [ a foaf:Organization ;
                    foaf:name "Signatu AS" ] ;
            foaf:homepage "https://www.linkedin.com/in/georg-philip-krog-a2a278104/" ;
            foaf:name "Georg P. Krog" ],
        _:person-harshvardhan-j-pandit,
        [ a dct:Agent,
                foaf:Person ;
            scoro:hasORCID "0009-0006-4623-1463" ;
            org:memberOf [ a foaf:Organization ;
                    foaf:name "University of Koblenz" ] ;
            foaf:name "Julian Flake" ],
        [ a dct:Agent,
                foaf:Person ;
            scoro:hasORCID "0000-0003-0770-2737" ;
            org:memberOf [ a foaf:Organization ;
                    foaf:name "Uniphar PLC" ] ;
            foaf:name "Paul Ryan" ] ;
    dct:description "Extension to the Data Privacy Vocabulary (DPV) providing concepts for representing information about technologies and its provision"@en ;
    dct:hasVersion tech-owl: ;
    dct:identifier "https://w3id.org/dpv/tech" ;
    dct:issued "2024-05-31"@en ;
    dct:license <https://www.w3.org/copyright/document-license-2023/> ;
    dct:modified "2025-08-01"@en ;
    dct:publisher <https://www.w3.org/> ;
    dct:source <https://www.w3.org/groups/cg/dpvcg/> ;
    dct:title "Technology Concepts"@en ;
    bibo:doi "10.5281/zenodo.12505841" ;
    bibo:status "http://purl.org/ontology/bibo/status/published" ;
    vann:preferredNamespacePrefix "tech" ;
    vann:preferredNamespaceUri "https://w3id.org/dpv/tech#" ;
    rdfs:Label "TECH"@en ;
    owl:versionIRI <https://w3id.org/dpv/2.2/tech/owl#> ;
    owl:versionInfo "2.2" ;
    profile:hasResource <https://w3id.org/dpv/examples>,
        <https://w3id.org/dpv/guides>,
        <https://w3id.org/dpv/primer>,
        tech-owl:serialisation-html,
        tech-owl:serialisation-jsonld,
        tech-owl:serialisation-n3,
        tech-owl:serialisation-rdf,
        tech-owl:serialisation-ttl ;
    profile:isProfileOf <http://www.w3.org/2002/07/owl>,
        <https://w3id.org/dpv/owl>,
        tech-owl: ;
    foaf:logo <https://w3id.org/dpv/media/logo.png> ;
    schema:version "2.2" .

_:org-adapt-centre-trinity-college-dublin a foaf:Organization ;
    foaf:name "ADAPT Centre, Trinity College Dublin" .

_:org-ai-accountability-lab-aial-trinity-college-dublin a foaf:Organization ;
    foaf:name "AI Accountability Lab (AIAL), Trinity College Dublin" .

_:person-delaram-golpayegani a dct:Agent,
        foaf:Person ;
    scoro:hasORCID "0000-0002-1208-186X" ;
    org:memberOf _:org-adapt-centre-trinity-college-dublin ;
    foaf:name "Delaram Golpayegani" .

_:person-harshvardhan-j-pandit a dct:Agent,
        foaf:Person ;
    scoro:hasORCID "0000-0002-5068-3714" ;
    org:memberOf _:org-ai-accountability-lab-aial-trinity-college-dublin ;
    foaf:homepage "https://harshp.com/" ;
    foaf:name "Harshvardhan J. Pandit" .

