<?xml version="1.0" encoding="utf-8"?>
<rdf:RDF
   xmlns:bibo="http://purl.org/ontology/bibo/"
   xmlns:dct="http://purl.org/dc/terms/"
   xmlns:foaf="http://xmlns.com/foaf/0.1/"
   xmlns:org="http://www.w3.org/ns/org#"
   xmlns:owl="http://www.w3.org/2002/07/owl#"
   xmlns:profile="http://www.w3.org/ns/dx/prof/"
   xmlns:rdf="http://www.w3.org/1999/02/22-rdf-syntax-ns#"
   xmlns:rdfs="http://www.w3.org/2000/01/rdf-schema#"
   xmlns:schema="https://schema.org/"
   xmlns:scoro="http://purl.org/spar/scoro/"
   xmlns:skos="http://www.w3.org/2004/02/skos/core#"
   xmlns:sw="http://www.w3.org/2003/06/sw-vocab-status/ns#"
   xmlns:vann="http://purl.org/vocab/vann/"
>
  <rdf:Description rdf:about="https://w3id.org/dpv/legal/eu/gdpr#SuitabilityAssessment">
    <rdf:type rdf:resource="http://www.w3.org/2004/02/skos/core#Concept"/>
    <rdf:type rdf:resource="http://www.w3.org/2000/01/rdf-schema#Class"/>
    <rdf:type rdf:resource="https://w3id.org/dpv#OrganisationalMeasure"/>
    <skos:prefLabel xml:lang="en">Suitability Assessment</skos:prefLabel>
    <skos:definition xml:lang="en">An assessment of whether the processing of personal data is suitable to achieve the stated aims</skos:definition>
    <skos:broader rdf:resource="https://w3id.org/dpv#Assessment"/>
    <skos:broader rdf:resource="https://w3id.org/dpv/legal/eu/gdpr#ProportionalityAssessment"/>
    <skos:scopeNote xml:lang="en">While Suitability Assessment can be carried out on its own, it is an integral part of the Proportionality Assessment process</skos:scopeNote>
    <dct:created rdf:datatype="http://www.w3.org/2001/XMLSchema#date">2026-02-06</dct:created>
    <dct:contributor rdf:nodeID="person-efstratios-koulierakis"/>
    <sw:term_status xml:lang="en">accepted</sw:term_status>
    <rdfs:isDefinedBy rdf:resource="https://w3id.org/dpv/legal/eu/gdpr#"/>
    <skos:inScheme rdf:resource="https://w3id.org/dpv/legal/eu/gdpr#proportionality-classes"/>
  </rdf:Description>
  <rdf:Description rdf:about="https://w3id.org/dpv/legal/eu/gdpr#serialisation-n3">
    <rdf:type rdf:resource="http://www.w3.org/ns/dx/prof/ResourceDescriptor"/>
    <profile:hasRole rdf:resource="http://www.w3.org/ns/dx/prof/role/vocabulary"/>
    <profile:hasArtifact rdf:resource="https://w3id.org/dpv/legal/eu/gdpr/eu-gdpr.n3"/>
    <dct:format rdf:resource="https://www.iana.org/assignments/media-types/text/n3"/>
    <dct:conformsTo rdf:resource="https://www.w3.org/TeamSubmission/n3/"/>
    <dct:title>EU General Data Protection Regulation (GDPR) - N3 serialisation</dct:title>
  </rdf:Description>
  <rdf:Description rdf:nodeID="person-georg-p-krog">
    <rdf:type rdf:resource="http://xmlns.com/foaf/0.1/Person"/>
    <rdf:type rdf:resource="http://purl.org/dc/terms/Agent"/>
    <foaf:name>Georg P. Krog</foaf:name>
    <foaf:homepage>https://www.linkedin.com/in/georg-philip-krog-a2a278104/</foaf:homepage>
    <org:memberOf rdf:nodeID="org-signatu-as"/>
  </rdf:Description>
  <rdf:Description rdf:about="https://w3id.org/dpv/legal/eu/gdpr#ProportionalityStatus">
    <rdf:type rdf:resource="http://www.w3.org/2004/02/skos/core#Concept"/>
    <rdf:type rdf:resource="http://www.w3.org/2000/01/rdf-schema#Class"/>
    <rdf:type rdf:resource="https://w3id.org/dpv#Status"/>
    <skos:prefLabel xml:lang="en">Proportionality Status</skos:prefLabel>
    <skos:definition xml:lang="en">Status indicating whether the specific activity or context is proportionate</skos:definition>
    <skos:broader rdf:resource="https://w3id.org/dpv#Status"/>
    <dct:created rdf:datatype="http://www.w3.org/2001/XMLSchema#date">2025-10-10</dct:created>
    <dct:contributor rdf:nodeID="person-efstratios-koulierakis"/>
    <dct:contributor rdf:nodeID="person-georg-p-krog"/>
    <dct:contributor rdf:nodeID="person-harshvardhan-j-pandit"/>
    <sw:term_status xml:lang="en">accepted</sw:term_status>
    <rdfs:isDefinedBy rdf:resource="https://w3id.org/dpv/legal/eu/gdpr#"/>
    <skos:inScheme rdf:resource="https://w3id.org/dpv/legal/eu/gdpr#proportionality-classes"/>
  </rdf:Description>
  <rdf:Description rdf:about="https://w3id.org/dpv/examples">
    <rdf:type rdf:resource="http://www.w3.org/ns/dx/prof/ResourceDescriptor"/>
    <profile:hasRole rdf:resource="http://www.w3.org/ns/dx/prof/role/guidance"/>
    <profile:hasArtifact rdf:resource="https://w3id.org/dpv/examples"/>
    <dct:title>Examples</dct:title>
    <dct:format rdf:resource="https://www.iana.org/assignments/media-types/text/html"/>
    <dct:conformsTo rdf:resource="https://www.w3.org/TR/html/"/>
  </rdf:Description>
  <rdf:Description rdf:about="https://w3id.org/dpv/legal/eu/gdpr#BalancingTest">
    <rdf:type rdf:resource="http://www.w3.org/2004/02/skos/core#Concept"/>
    <rdf:type rdf:resource="http://www.w3.org/2000/01/rdf-schema#Class"/>
    <rdf:type rdf:resource="https://w3id.org/dpv#OrganisationalMeasure"/>
    <skos:prefLabel xml:lang="en">Balancing Test</skos:prefLabel>
    <skos:definition xml:lang="en">An assessment of whether the individual's interests override the interests of the controller</skos:definition>
    <skos:broader rdf:resource="https://w3id.org/dpv#Assessment"/>
    <skos:broader rdf:resource="https://w3id.org/dpv/legal/eu/gdpr#ProportionalityAssessment"/>
    <skos:scopeNote xml:lang="en">While Balancing Test can be conducted on its own, it is an integral part of the Proportionality Assessment process</skos:scopeNote>
    <dct:created rdf:datatype="http://www.w3.org/2001/XMLSchema#date">2025-10-10</dct:created>
    <dct:contributor rdf:nodeID="person-efstratios-koulierakis"/>
    <dct:contributor rdf:nodeID="person-georg-p-krog"/>
    <dct:contributor rdf:nodeID="person-harshvardhan-j-pandit"/>
    <sw:term_status xml:lang="en">accepted</sw:term_status>
    <rdfs:isDefinedBy rdf:resource="https://w3id.org/dpv/legal/eu/gdpr#"/>
    <skos:inScheme rdf:resource="https://w3id.org/dpv/legal/eu/gdpr#proportionality-classes"/>
  </rdf:Description>
  <rdf:Description rdf:about="https://w3id.org/dpv/legal/eu/gdpr#Disproportionate">
    <rdf:type rdf:resource="http://www.w3.org/2004/02/skos/core#Concept"/>
    <rdf:type rdf:resource="http://www.w3.org/2000/01/rdf-schema#Class"/>
    <rdf:type rdf:resource="https://w3id.org/dpv/legal/eu/gdpr#ProportionalityStatus"/>
    <skos:prefLabel xml:lang="en">Disproportionate</skos:prefLabel>
    <skos:definition xml:lang="en">Status representing the activity or context is disproportionate i.e. it is not proportionate</skos:definition>
    <skos:broader rdf:resource="https://w3id.org/dpv/legal/eu/gdpr#ProportionalityStatus"/>
    <skos:scopeNote xml:lang="en">A Disproportinate status indicates that the process should not be continued as it risks impacting the rights of the data subject in an unacceptable manner</skos:scopeNote>
    <dct:created rdf:datatype="http://www.w3.org/2001/XMLSchema#date">2025-10-10</dct:created>
    <dct:contributor rdf:nodeID="person-efstratios-koulierakis"/>
    <dct:contributor rdf:nodeID="person-georg-p-krog"/>
    <dct:contributor rdf:nodeID="person-harshvardhan-j-pandit"/>
    <sw:term_status xml:lang="en">accepted</sw:term_status>
    <rdfs:isDefinedBy rdf:resource="https://w3id.org/dpv/legal/eu/gdpr#"/>
    <skos:inScheme rdf:resource="https://w3id.org/dpv/legal/eu/gdpr#proportionality-classes"/>
  </rdf:Description>
  <rdf:Description rdf:nodeID="person-beatriz-esteves">
    <rdf:type rdf:resource="http://xmlns.com/foaf/0.1/Person"/>
    <rdf:type rdf:resource="http://purl.org/dc/terms/Agent"/>
    <foaf:name>Beatriz Esteves</foaf:name>
    <scoro:hasORCID>0000-0003-0259-7560</scoro:hasORCID>
    <foaf:homepage>https://w3id.org/people/besteves</foaf:homepage>
    <org:memberOf rdf:nodeID="org-idlab-imec-ghent-university"/>
  </rdf:Description>
  <rdf:Description rdf:about="https://w3id.org/dpv/legal/eu/gdpr#NecessityAssessment">
    <rdf:type rdf:resource="http://www.w3.org/2004/02/skos/core#Concept"/>
    <rdf:type rdf:resource="http://www.w3.org/2000/01/rdf-schema#Class"/>
    <rdf:type rdf:resource="https://w3id.org/dpv#OrganisationalMeasure"/>
    <skos:prefLabel xml:lang="en">Necessity Assessment</skos:prefLabel>
    <skos:definition xml:lang="en">An assessment of whether the processing of personal data is necessary to achieve the stated aims, where necessary indicates a lack of other means which could have been used instead</skos:definition>
    <skos:broader rdf:resource="https://w3id.org/dpv#Assessment"/>
    <skos:broader rdf:resource="https://w3id.org/dpv/legal/eu/gdpr#ProportionalityAssessment"/>
    <skos:scopeNote xml:lang="en">While Necessity can be assessed on its own, it is an integral part of the Proportionality Assessment process</skos:scopeNote>
    <dct:created rdf:datatype="http://www.w3.org/2001/XMLSchema#date">2025-10-10</dct:created>
    <dct:contributor rdf:nodeID="person-efstratios-koulierakis"/>
    <dct:contributor rdf:nodeID="person-georg-p-krog"/>
    <dct:contributor rdf:nodeID="person-harshvardhan-j-pandit"/>
    <sw:term_status xml:lang="en">accepted</sw:term_status>
    <rdfs:isDefinedBy rdf:resource="https://w3id.org/dpv/legal/eu/gdpr#"/>
    <skos:inScheme rdf:resource="https://w3id.org/dpv/legal/eu/gdpr#proportionality-classes"/>
  </rdf:Description>
  <rdf:Description rdf:about="https://w3id.org/dpv/legal/eu/gdpr#Proportionate">
    <rdf:type rdf:resource="http://www.w3.org/2004/02/skos/core#Concept"/>
    <rdf:type rdf:resource="http://www.w3.org/2000/01/rdf-schema#Class"/>
    <rdf:type rdf:resource="https://w3id.org/dpv/legal/eu/gdpr#ProportionalityStatus"/>
    <skos:prefLabel xml:lang="en">Proportionate</skos:prefLabel>
    <skos:definition xml:lang="en">Status representing the activity or context is proportionate</skos:definition>
    <skos:broader rdf:resource="https://w3id.org/dpv/legal/eu/gdpr#ProportionalityStatus"/>
    <dct:created rdf:datatype="http://www.w3.org/2001/XMLSchema#date">2025-10-10</dct:created>
    <dct:contributor rdf:nodeID="person-efstratios-koulierakis"/>
    <dct:contributor rdf:nodeID="person-georg-p-krog"/>
    <dct:contributor rdf:nodeID="person-harshvardhan-j-pandit"/>
    <sw:term_status xml:lang="en">accepted</sw:term_status>
    <rdfs:isDefinedBy rdf:resource="https://w3id.org/dpv/legal/eu/gdpr#"/>
    <skos:inScheme rdf:resource="https://w3id.org/dpv/legal/eu/gdpr#proportionality-classes"/>
  </rdf:Description>
  <rdf:Description rdf:about="https://w3id.org/dpv/legal/eu/gdpr">
    <rdf:type rdf:resource="http://www.w3.org/2002/07/owl#Ontology"/>
    <rdf:type rdf:resource="http://www.w3.org/ns/dx/prof/Profile"/>
    <owl:versionIRI rdf:resource="https://w3id.org/dpv/2.3/legal/eu/gdpr"/>
    <dct:source rdf:resource="https://www.w3.org/groups/cg/dpvcg/"/>
    <dct:title xml:lang="en">EU General Data Protection Regulation (GDPR)</dct:title>
    <bibo:status>http://purl.org/ontology/bibo/status/published</bibo:status>
    <rdfs:Label xml:lang="en">EU-GDPR</rdfs:Label>
    <dct:description xml:lang="en">Extension to the Data Privacy Vocabulary (DPV) providing concepts for representing information associated with EU GDPR</dct:description>
    <dct:created xml:lang="en">2019-06-18</dct:created>
    <dct:issued xml:lang="en">2019-06-18</dct:issued>
    <dct:modified xml:lang="en">2026-02-25</dct:modified>
    <dct:creator rdf:nodeID="person-harshvardhan-j-pandit"/>
    <dct:creator rdf:nodeID="person-georg-p-krog"/>
    <dct:creator rdf:nodeID="person-paul-ryan"/>
    <dct:creator rdf:nodeID="person-beatriz-esteves"/>
    <dct:creator rdf:nodeID="person-efstratios-koulierakis"/>
    <schema:version>2.3</schema:version>
    <owl:versionInfo>2.3</owl:versionInfo>
    <dct:identifier>https://w3id.org/dpv/legal/eu/gdpr</dct:identifier>
    <dct:conformsTo>http://www.w3.org/2000/01/rdf-schema</dct:conformsTo>
    <dct:conformsTo>http://www.w3.org/2004/02/skos/core</dct:conformsTo>
    <bibo:doi>10.5281/zenodo.12505841</bibo:doi>
    <dct:bibliographicCitation>Harshvardhan J. Pandit, Beatriz Esteves, Georg P. Krog, Paul Ryan, Delaram Golpayegani, Julian Flake (2025) Data Privacy Vocabulary (DPV) – Version 2.0. In: Demartini, G., et al. The Semantic Web – ISWC 2024. ISWC 2024. Lecture Notes in Computer Science, vol 15233. Springer, Cham. https://doi.org/10.1007/978-3-031-77847-6_10</dct:bibliographicCitation>
    <dct:publisher rdf:resource="https://www.w3.org/"/>
    <foaf:logo rdf:resource="https://w3id.org/dpv/media/logo.png"/>
    <dct:contributor rdf:nodeID="person-harshvardhan-j-pandit"/>
    <dct:contributor rdf:nodeID="person-efstratios-koulierakis"/>
    <dct:contributor rdf:nodeID="person-georg-p-krog"/>
    <dct:license rdf:resource="https://www.w3.org/copyright/document-license-2023/"/>
    <vann:preferredNamespacePrefix>eu-gdpr</vann:preferredNamespacePrefix>
    <vann:preferredNamespaceUri>https://w3id.org/dpv/legal/eu/gdpr#</vann:preferredNamespaceUri>
    <profile:isProfileOf rdf:resource="http://www.w3.org/2000/01/rdf-schema#"/>
    <profile:isProfileOf rdf:resource="http://www.w3.org/2004/02/skos/core#"/>
    <profile:isProfileOf rdf:resource="https://w3id.org/dpv"/>
    <profile:hasResource rdf:resource="https://w3id.org/dpv/primer"/>
    <profile:hasResource rdf:resource="https://w3id.org/dpv/guides"/>
    <profile:hasResource rdf:resource="https://w3id.org/dpv/examples"/>
    <profile:hasResource rdf:resource="https://w3id.org/dpv/legal/eu/gdpr#serialisation-html"/>
    <profile:hasResource rdf:resource="https://w3id.org/dpv/legal/eu/gdpr#serialisation-rdf"/>
    <profile:hasResource rdf:resource="https://w3id.org/dpv/legal/eu/gdpr#serialisation-ttl"/>
    <profile:hasResource rdf:resource="https://w3id.org/dpv/legal/eu/gdpr#serialisation-n3"/>
    <profile:hasResource rdf:resource="https://w3id.org/dpv/legal/eu/gdpr#serialisation-jsonld"/>
  </rdf:Description>
  <rdf:Description rdf:nodeID="org-signatu-as">
    <rdf:type rdf:resource="http://xmlns.com/foaf/0.1/Organization"/>
    <foaf:name>Signatu AS</foaf:name>
  </rdf:Description>
  <rdf:Description rdf:about="https://w3id.org/dpv/legal/eu/gdpr#serialisation-html">
    <rdf:type rdf:resource="http://www.w3.org/ns/dx/prof/ResourceDescriptor"/>
    <profile:hasRole rdf:resource="http://www.w3.org/ns/dx/prof/role/specification"/>
    <profile:hasArtifact rdf:resource="https://w3id.org/dpv/legal/eu/gdpr/eu-gdpr.html"/>
    <dct:format rdf:resource="https://www.iana.org/assignments/media-types/text/html"/>
    <dct:conformsTo rdf:resource="https://www.w3.org/TR/html/"/>
    <dct:title>EU General Data Protection Regulation (GDPR) - HTML serialisation</dct:title>
  </rdf:Description>
  <rdf:Description rdf:nodeID="person-harshvardhan-j-pandit">
    <rdf:type rdf:resource="http://xmlns.com/foaf/0.1/Person"/>
    <rdf:type rdf:resource="http://purl.org/dc/terms/Agent"/>
    <foaf:name>Harshvardhan J. Pandit</foaf:name>
    <scoro:hasORCID>0000-0002-5068-3714</scoro:hasORCID>
    <foaf:homepage>https://harshp.com/</foaf:homepage>
    <org:memberOf rdf:nodeID="org-ai-accountability-lab-aial-trinity-college-dublin"/>
  </rdf:Description>
  <rdf:Description rdf:about="https://w3id.org/dpv/legal/eu/gdpr#serialisation-ttl">
    <rdf:type rdf:resource="http://www.w3.org/ns/dx/prof/ResourceDescriptor"/>
    <profile:hasRole rdf:resource="http://www.w3.org/ns/dx/prof/role/vocabulary"/>
    <profile:hasArtifact rdf:resource="https://w3id.org/dpv/legal/eu/gdpr/eu-gdpr.ttl"/>
    <dct:format rdf:resource="https://www.iana.org/assignments/media-types/text/turtle"/>
    <dct:conformsTo rdf:resource="https://www.w3.org/TR/turtle/"/>
    <dct:title>EU General Data Protection Regulation (GDPR) - Turtle serialisation</dct:title>
  </rdf:Description>
  <rdf:Description rdf:nodeID="org-idlab-imec-ghent-university">
    <rdf:type rdf:resource="http://xmlns.com/foaf/0.1/Organization"/>
    <foaf:name>IDLab, IMEC, Ghent University</foaf:name>
  </rdf:Description>
  <rdf:Description rdf:nodeID="person-paul-ryan">
    <rdf:type rdf:resource="http://xmlns.com/foaf/0.1/Person"/>
    <rdf:type rdf:resource="http://purl.org/dc/terms/Agent"/>
    <foaf:name>Paul Ryan</foaf:name>
    <scoro:hasORCID>0000-0003-0770-2737</scoro:hasORCID>
    <org:memberOf rdf:nodeID="org-uniphar-plc"/>
  </rdf:Description>
  <rdf:Description rdf:about="https://w3id.org/dpv/guides">
    <rdf:type rdf:resource="http://www.w3.org/ns/dx/prof/ResourceDescriptor"/>
    <profile:hasRole rdf:resource="http://www.w3.org/ns/dx/prof/role/guidance"/>
    <profile:hasArtifact rdf:resource="https://w3id.org/dpv/guides"/>
    <dct:title>Guides for Data Privacy Vocabulary</dct:title>
    <dct:format rdf:resource="https://www.iana.org/assignments/media-types/text/html"/>
    <dct:conformsTo rdf:resource="https://www.w3.org/TR/html/"/>
  </rdf:Description>
  <rdf:Description rdf:about="https://w3id.org/dpv/legal/eu/gdpr#ProportionalityAssessment">
    <rdf:type rdf:resource="http://www.w3.org/2004/02/skos/core#Concept"/>
    <rdf:type rdf:resource="http://www.w3.org/2000/01/rdf-schema#Class"/>
    <rdf:type rdf:resource="https://w3id.org/dpv#OrganisationalMeasure"/>
    <skos:prefLabel xml:lang="en">Proportionality Assessment</skos:prefLabel>
    <skos:definition xml:lang="en">Proportionality is a general principle of EU law, which when applied for the GDPR requires striking a balance between the processing of personal data and the resulting impacts on rights. More simply, the processing should not result in a disproportionate impact on rights</skos:definition>
    <skos:broader rdf:resource="https://w3id.org/dpv#ImpactAssessment"/>
    <skos:scopeNote xml:lang="en">The assessment of proportionality requires an assessment of suitability (represented by `eu-gdpr:SuitabilityAssessment`), necessity (represented by `eu-gdpr:NecessityAssessment`), and a balancing test (represented by `eu-gdpr:BalancingTest`). The outcome of the proportionality assessment is represented as an instance of `eu-gdpr:ProportionalityStatus`</skos:scopeNote>
    <dct:created rdf:datatype="http://www.w3.org/2001/XMLSchema#date">2025-10-10</dct:created>
    <dct:contributor rdf:nodeID="person-efstratios-koulierakis"/>
    <dct:contributor rdf:nodeID="person-georg-p-krog"/>
    <dct:contributor rdf:nodeID="person-harshvardhan-j-pandit"/>
    <sw:term_status xml:lang="en">accepted</sw:term_status>
    <rdfs:isDefinedBy rdf:resource="https://w3id.org/dpv/legal/eu/gdpr#"/>
    <skos:inScheme rdf:resource="https://w3id.org/dpv/legal/eu/gdpr#proportionality-classes"/>
  </rdf:Description>
  <rdf:Description rdf:nodeID="org-uniphar-plc">
    <rdf:type rdf:resource="http://xmlns.com/foaf/0.1/Organization"/>
    <foaf:name>Uniphar PLC</foaf:name>
  </rdf:Description>
  <rdf:Description rdf:about="https://w3id.org/dpv/primer">
    <profile:hasRole rdf:resource="http://www.w3.org/ns/dx/prof/role/guidance"/>
    <rdf:type rdf:resource="http://www.w3.org/ns/dx/prof/ResourceDescriptor"/>
    <profile:hasArtifact rdf:resource="https://w3id.org/dpv/primer"/>
    <dct:title>Primer for Data Privacy Vocabulary</dct:title>
    <dct:format rdf:resource="https://www.iana.org/assignments/media-types/text/html"/>
    <dct:conformsTo rdf:resource="https://www.w3.org/TR/html/"/>
  </rdf:Description>
  <rdf:Description rdf:about="https://w3id.org/dpv/legal/eu/gdpr#serialisation-rdf">
    <rdf:type rdf:resource="http://www.w3.org/ns/dx/prof/ResourceDescriptor"/>
    <profile:hasRole rdf:resource="http://www.w3.org/ns/dx/prof/role/vocabulary"/>
    <profile:hasArtifact rdf:resource="https://w3id.org/dpv/legal/eu/gdpr/eu-gdpr.rdf"/>
    <dct:format rdf:resource="https://www.iana.org/assignments/media-types/application/rdf+xml"/>
    <dct:conformsTo rdf:resource="http://www.w3.org/1999/02/22-rdf-syntax-ns#"/>
    <dct:title>EU General Data Protection Regulation (GDPR) - RDF/XML serialisation</dct:title>
  </rdf:Description>
  <rdf:Description rdf:about="https://w3id.org/dpv/legal/eu/gdpr#serialisation-jsonld">
    <rdf:type rdf:resource="http://www.w3.org/ns/dx/prof/ResourceDescriptor"/>
    <profile:hasRole rdf:resource="http://www.w3.org/ns/dx/prof/role/vocabulary"/>
    <profile:hasArtifact rdf:resource="https://w3id.org/dpv/legal/eu/gdpr/eu-gdpr.jsonld"/>
    <dct:format rdf:resource="https://www.iana.org/assignments/media-types/application/ld+json"/>
    <dct:conformsTo rdf:resource="https://www.w3.org/TR/json-ld11/"/>
    <dct:title>EU General Data Protection Regulation (GDPR) - JSON-LD serialisation</dct:title>
  </rdf:Description>
  <rdf:Description rdf:nodeID="person-efstratios-koulierakis">
    <rdf:type rdf:resource="http://xmlns.com/foaf/0.1/Person"/>
    <rdf:type rdf:resource="http://purl.org/dc/terms/Agent"/>
    <foaf:name>Efstratios Koulierakis</foaf:name>
    <org:memberOf rdf:nodeID="org-university-of-athens"/>
  </rdf:Description>
  <rdf:Description rdf:nodeID="org-ai-accountability-lab-aial-trinity-college-dublin">
    <rdf:type rdf:resource="http://xmlns.com/foaf/0.1/Organization"/>
    <foaf:name>AI Accountability Lab (AIAL), Trinity College Dublin</foaf:name>
  </rdf:Description>
  <rdf:Description rdf:nodeID="org-university-of-athens">
    <rdf:type rdf:resource="http://xmlns.com/foaf/0.1/Organization"/>
    <foaf:name>University of Athens</foaf:name>
  </rdf:Description>
  <rdf:Description rdf:about="https://w3id.org/dpv/legal/eu/gdpr#proportionality-classes">
    <rdf:type rdf:resource="http://www.w3.org/2004/02/skos/core#ConceptScheme"/>
  </rdf:Description>
</rdf:RDF>
