@prefix bibo: <http://purl.org/ontology/bibo/> .
@prefix dct: <http://purl.org/dc/terms/> .
@prefix dpv: <https://w3id.org/dpv#> .
@prefix eu-gdpr: <https://w3id.org/dpv/legal/eu/gdpr#> .
@prefix foaf: <http://xmlns.com/foaf/0.1/> .
@prefix org: <http://www.w3.org/ns/org#> .
@prefix owl: <http://www.w3.org/2002/07/owl#> .
@prefix profile: <http://www.w3.org/ns/dx/prof/> .
@prefix rdf: <http://www.w3.org/1999/02/22-rdf-syntax-ns#> .
@prefix rdfs: <http://www.w3.org/2000/01/rdf-schema#> .
@prefix role: <http://www.w3.org/ns/dx/prof/role/> .
@prefix schema: <https://schema.org/> .
@prefix scoro: <http://purl.org/spar/scoro/> .
@prefix skos: <http://www.w3.org/2004/02/skos/core#> .
@prefix sw: <http://www.w3.org/2003/06/sw-vocab-status/ns#> .
@prefix vann: <http://purl.org/vocab/vann/> .
@prefix xsd: <http://www.w3.org/2001/XMLSchema#> .

eu-gdpr:BalancingTest a rdfs:Class,
        skos:Concept,
        dpv:OrganisationalMeasure ;
    dct:contributor _:person-efstratios-koulierakis,
        _:person-georg-p-krog,
        _:person-harshvardhan-j-pandit ;
    dct:created "2025-10-10"^^xsd:date ;
    rdfs:isDefinedBy eu-gdpr: ;
    sw:term_status "accepted"@en ;
    skos:broader dpv:Assessment,
        eu-gdpr:ProportionalityAssessment ;
    skos:definition "An assessment of whether the individual's interests override the interests of the controller"@en ;
    skos:inScheme eu-gdpr:proportionality-classes ;
    skos:prefLabel "Balancing Test"@en ;
    skos:scopeNote "While Balancing Test can be conducted on its own, it is an integral part of the Proportionality Assessment process"@en .

eu-gdpr:Disproportionate a rdfs:Class,
        skos:Concept,
        eu-gdpr:ProportionalityStatus ;
    dct:contributor _:person-efstratios-koulierakis,
        _:person-georg-p-krog,
        _:person-harshvardhan-j-pandit ;
    dct:created "2025-10-10"^^xsd:date ;
    rdfs:isDefinedBy eu-gdpr: ;
    sw:term_status "accepted"@en ;
    skos:broader eu-gdpr:ProportionalityStatus ;
    skos:definition "Status representing the activity or context is disproportionate i.e. it is not proportionate"@en ;
    skos:inScheme eu-gdpr:proportionality-classes ;
    skos:prefLabel "Disproportionate"@en ;
    skos:scopeNote "A Disproportinate status indicates that the process should not be continued as it risks impacting the rights of the data subject in an unacceptable manner"@en .

eu-gdpr:NecessityAssessment a rdfs:Class,
        skos:Concept,
        dpv:OrganisationalMeasure ;
    dct:contributor _:person-efstratios-koulierakis,
        _:person-georg-p-krog,
        _:person-harshvardhan-j-pandit ;
    dct:created "2025-10-10"^^xsd:date ;
    rdfs:isDefinedBy eu-gdpr: ;
    sw:term_status "accepted"@en ;
    skos:broader dpv:Assessment,
        eu-gdpr:ProportionalityAssessment ;
    skos:definition "An assessment of whether the processing of personal data is necessary to achieve the stated aims, where necessary indicates a lack of other means which could have been used instead"@en ;
    skos:inScheme eu-gdpr:proportionality-classes ;
    skos:prefLabel "Necessity Assessment"@en ;
    skos:scopeNote "While Necessity can be assessed on its own, it is an integral part of the Proportionality Assessment process"@en .

eu-gdpr:ProportionalityAssessment a rdfs:Class,
        skos:Concept,
        dpv:OrganisationalMeasure ;
    dct:contributor _:person-efstratios-koulierakis,
        _:person-georg-p-krog,
        _:person-harshvardhan-j-pandit ;
    dct:created "2025-10-10"^^xsd:date ;
    rdfs:isDefinedBy eu-gdpr: ;
    sw:term_status "accepted"@en ;
    skos:broader dpv:ImpactAssessment ;
    skos:definition "Proportionality is a general principle of EU law, which when applied for the GDPR requires striking a balance between the processing of personal data and the resulting impacts on rights. More simply, the processing should not result in a disproportionate impact on rights"@en ;
    skos:inScheme eu-gdpr:proportionality-classes ;
    skos:prefLabel "Proportionality Assessment"@en ;
    skos:scopeNote "The assessment of proportionality requires an assessment of suitability (represented by `eu-gdpr:SuitabilityAssessment`), necessity (represented by `eu-gdpr:NecessityAssessment`), and a balancing test (represented by `eu-gdpr:BalancingTest`). The outcome of the proportionality assessment is represented as an instance of `eu-gdpr:ProportionalityStatus`"@en .

eu-gdpr:ProportionalityStatus a rdfs:Class,
        skos:Concept,
        dpv:Status ;
    dct:contributor _:person-efstratios-koulierakis,
        _:person-georg-p-krog,
        _:person-harshvardhan-j-pandit ;
    dct:created "2025-10-10"^^xsd:date ;
    rdfs:isDefinedBy eu-gdpr: ;
    sw:term_status "accepted"@en ;
    skos:broader dpv:Status ;
    skos:definition "Status indicating whether the specific activity or context is proportionate"@en ;
    skos:inScheme eu-gdpr:proportionality-classes ;
    skos:prefLabel "Proportionality Status"@en .

eu-gdpr:Proportionate a rdfs:Class,
        skos:Concept,
        eu-gdpr:ProportionalityStatus ;
    dct:contributor _:person-efstratios-koulierakis,
        _:person-georg-p-krog,
        _:person-harshvardhan-j-pandit ;
    dct:created "2025-10-10"^^xsd:date ;
    rdfs:isDefinedBy eu-gdpr: ;
    sw:term_status "accepted"@en ;
    skos:broader eu-gdpr:ProportionalityStatus ;
    skos:definition "Status representing the activity or context is proportionate"@en ;
    skos:inScheme eu-gdpr:proportionality-classes ;
    skos:prefLabel "Proportionate"@en .

eu-gdpr:SuitabilityAssessment a rdfs:Class,
        skos:Concept,
        dpv:OrganisationalMeasure ;
    dct:contributor _:person-efstratios-koulierakis ;
    dct:created "2026-02-06"^^xsd:date ;
    rdfs:isDefinedBy eu-gdpr: ;
    sw:term_status "accepted"@en ;
    skos:broader dpv:Assessment,
        eu-gdpr:ProportionalityAssessment ;
    skos:definition "An assessment of whether the processing of personal data is suitable to achieve the stated aims"@en ;
    skos:inScheme eu-gdpr:proportionality-classes ;
    skos:prefLabel "Suitability Assessment"@en ;
    skos:scopeNote "While Suitability Assessment can be carried out on its own, it is an integral part of the Proportionality Assessment process"@en .

<https://w3id.org/dpv/legal/eu/gdpr> a owl:Ontology,
        profile:Profile ;
    dct:bibliographicCitation "Harshvardhan J. Pandit, Beatriz Esteves, Georg P. Krog, Paul Ryan, Delaram Golpayegani, Julian Flake (2025) Data Privacy Vocabulary (DPV) – Version 2.0. In: Demartini, G., et al. The Semantic Web – ISWC 2024. ISWC 2024. Lecture Notes in Computer Science, vol 15233. Springer, Cham. https://doi.org/10.1007/978-3-031-77847-6_10" ;
    dct:conformsTo "http://www.w3.org/2000/01/rdf-schema",
        "http://www.w3.org/2004/02/skos/core" ;
    dct:contributor _:person-efstratios-koulierakis,
        _:person-georg-p-krog,
        _:person-harshvardhan-j-pandit ;
    dct:created "2019-06-18"@en ;
    dct:creator [ a dct:Agent,
                foaf:Person ;
            scoro:hasORCID "0000-0003-0259-7560" ;
            org:memberOf [ a foaf:Organization ;
                    foaf:name "IDLab, IMEC, Ghent University" ] ;
            foaf:homepage "https://w3id.org/people/besteves" ;
            foaf:name "Beatriz Esteves" ],
        _:person-efstratios-koulierakis,
        _:person-georg-p-krog,
        _:person-harshvardhan-j-pandit,
        [ a dct:Agent,
                foaf:Person ;
            scoro:hasORCID "0000-0003-0770-2737" ;
            org:memberOf [ a foaf:Organization ;
                    foaf:name "Uniphar PLC" ] ;
            foaf:name "Paul Ryan" ] ;
    dct:description "Extension to the Data Privacy Vocabulary (DPV) providing concepts for representing information associated with EU GDPR"@en ;
    dct:identifier "https://w3id.org/dpv/legal/eu/gdpr" ;
    dct:issued "2019-06-18"@en ;
    dct:license <https://www.w3.org/copyright/document-license-2023/> ;
    dct:modified "2026-02-25"@en ;
    dct:publisher <https://www.w3.org/> ;
    dct:source <https://www.w3.org/groups/cg/dpvcg/> ;
    dct:title "EU General Data Protection Regulation (GDPR)"@en ;
    bibo:doi "10.5281/zenodo.12505841" ;
    bibo:status "http://purl.org/ontology/bibo/status/published" ;
    vann:preferredNamespacePrefix "eu-gdpr" ;
    vann:preferredNamespaceUri "https://w3id.org/dpv/legal/eu/gdpr#" ;
    rdfs:Label "EU-GDPR"@en ;
    owl:versionIRI <https://w3id.org/dpv/2.3/legal/eu/gdpr> ;
    owl:versionInfo "2.3" ;
    profile:hasResource <https://w3id.org/dpv/examples>,
        <https://w3id.org/dpv/guides>,
        eu-gdpr:serialisation-html,
        eu-gdpr:serialisation-jsonld,
        eu-gdpr:serialisation-n3,
        eu-gdpr:serialisation-rdf,
        eu-gdpr:serialisation-ttl,
        <https://w3id.org/dpv/primer> ;
    profile:isProfileOf rdfs:,
        skos:,
        <https://w3id.org/dpv> ;
    foaf:logo <https://w3id.org/dpv/media/logo.png> ;
    schema:version "2.3" .

eu-gdpr:serialisation-html a profile:ResourceDescriptor ;
    dct:conformsTo <https://www.w3.org/TR/html/> ;
    dct:format <https://www.iana.org/assignments/media-types/text/html> ;
    dct:title "EU General Data Protection Regulation (GDPR) - HTML serialisation" ;
    profile:hasArtifact <https://w3id.org/dpv/legal/eu/gdpr/eu-gdpr.html> ;
    profile:hasRole role:specification .

eu-gdpr:serialisation-jsonld a profile:ResourceDescriptor ;
    dct:conformsTo <https://www.w3.org/TR/json-ld11/> ;
    dct:format <https://www.iana.org/assignments/media-types/application/ld+json> ;
    dct:title "EU General Data Protection Regulation (GDPR) - JSON-LD serialisation" ;
    profile:hasArtifact <https://w3id.org/dpv/legal/eu/gdpr/eu-gdpr.jsonld> ;
    profile:hasRole role:vocabulary .

eu-gdpr:serialisation-n3 a profile:ResourceDescriptor ;
    dct:conformsTo <https://www.w3.org/TeamSubmission/n3/> ;
    dct:format <https://www.iana.org/assignments/media-types/text/n3> ;
    dct:title "EU General Data Protection Regulation (GDPR) - N3 serialisation" ;
    profile:hasArtifact <https://w3id.org/dpv/legal/eu/gdpr/eu-gdpr.n3> ;
    profile:hasRole role:vocabulary .

eu-gdpr:serialisation-rdf a profile:ResourceDescriptor ;
    dct:conformsTo rdf: ;
    dct:format <https://www.iana.org/assignments/media-types/application/rdf+xml> ;
    dct:title "EU General Data Protection Regulation (GDPR) - RDF/XML serialisation" ;
    profile:hasArtifact <https://w3id.org/dpv/legal/eu/gdpr/eu-gdpr.rdf> ;
    profile:hasRole role:vocabulary .

eu-gdpr:serialisation-ttl a profile:ResourceDescriptor ;
    dct:conformsTo <https://www.w3.org/TR/turtle/> ;
    dct:format <https://www.iana.org/assignments/media-types/text/turtle> ;
    dct:title "EU General Data Protection Regulation (GDPR) - Turtle serialisation" ;
    profile:hasArtifact <https://w3id.org/dpv/legal/eu/gdpr/eu-gdpr.ttl> ;
    profile:hasRole role:vocabulary .

<https://w3id.org/dpv/examples> a profile:ResourceDescriptor ;
    dct:conformsTo <https://www.w3.org/TR/html/> ;
    dct:format <https://www.iana.org/assignments/media-types/text/html> ;
    dct:title "Examples" ;
    profile:hasArtifact <https://w3id.org/dpv/examples> ;
    profile:hasRole role:guidance .

<https://w3id.org/dpv/guides> a profile:ResourceDescriptor ;
    dct:conformsTo <https://www.w3.org/TR/html/> ;
    dct:format <https://www.iana.org/assignments/media-types/text/html> ;
    dct:title "Guides for Data Privacy Vocabulary" ;
    profile:hasArtifact <https://w3id.org/dpv/guides> ;
    profile:hasRole role:guidance .

<https://w3id.org/dpv/primer> a profile:ResourceDescriptor ;
    dct:conformsTo <https://www.w3.org/TR/html/> ;
    dct:format <https://www.iana.org/assignments/media-types/text/html> ;
    dct:title "Primer for Data Privacy Vocabulary" ;
    profile:hasArtifact <https://w3id.org/dpv/primer> ;
    profile:hasRole role:guidance .

eu-gdpr:proportionality-classes a skos:ConceptScheme .

_:org-ai-accountability-lab-aial-trinity-college-dublin a foaf:Organization ;
    foaf:name "AI Accountability Lab (AIAL), Trinity College Dublin" .

_:org-signatu-as a foaf:Organization ;
    foaf:name "Signatu AS" .

_:org-university-of-athens a foaf:Organization ;
    foaf:name "University of Athens" .

_:person-georg-p-krog a dct:Agent,
        foaf:Person ;
    org:memberOf _:org-signatu-as ;
    foaf:homepage "https://www.linkedin.com/in/georg-philip-krog-a2a278104/" ;
    foaf:name "Georg P. Krog" .

_:person-harshvardhan-j-pandit a dct:Agent,
        foaf:Person ;
    scoro:hasORCID "0000-0002-5068-3714" ;
    org:memberOf _:org-ai-accountability-lab-aial-trinity-college-dublin ;
    foaf:homepage "https://harshp.com/" ;
    foaf:name "Harshvardhan J. Pandit" .

_:person-efstratios-koulierakis a dct:Agent,
        foaf:Person ;
    org:memberOf _:org-university-of-athens ;
    foaf:name "Efstratios Koulierakis" .

