@prefix bibo: <http://purl.org/ontology/bibo/> .
@prefix dct: <http://purl.org/dc/terms/> .
@prefix dpv-owl: <https://w3id.org/dpv/owl#> .
@prefix foaf: <http://xmlns.com/foaf/0.1/> .
@prefix org: <http://www.w3.org/ns/org#> .
@prefix owl: <http://www.w3.org/2002/07/owl#> .
@prefix profile: <http://www.w3.org/ns/dx/prof/> .
@prefix rdf: <http://www.w3.org/1999/02/22-rdf-syntax-ns#> .
@prefix rdfs: <http://www.w3.org/2000/01/rdf-schema#> .
@prefix role: <http://www.w3.org/ns/dx/prof/role/> .
@prefix schema: <https://schema.org/> .
@prefix scoro: <http://purl.org/spar/scoro/> .
@prefix sector-education-owl: <https://w3id.org/dpv/sector/education/owl#> .
@prefix skos: <http://www.w3.org/2004/02/skos/core#> .
@prefix sw: <http://www.w3.org/2003/06/sw-vocab-status/ns#> .
@prefix vann: <http://purl.org/vocab/vann/> .
@prefix xsd: <http://www.w3.org/2001/XMLSchema#> .

sector-education-owl:AccessManagement a rdfs:Class,
        owl:Class,
        dpv-owl:Purpose ;
    dct:created "2024-12-01"^^xsd:date ;
    rdfs:isDefinedBy sector-education-owl: ;
    rdfs:subClassOf sector-education-owl:EducationManagement ;
    sw:term_status "accepted"@en ;
    skos:definition "Purposes associated with determination and management of access to educational programs, resources, and services"@en ;
    skos:prefLabel "AccessManagement"@en .

sector-education-owl:EducationManagement a rdfs:Class,
        owl:Class,
        dpv-owl:Purpose ;
    dct:created "2024-12-01"^^xsd:date ;
    rdfs:isDefinedBy sector-education-owl: ;
    rdfs:subClassOf dpv-owl:Purpose ;
    sw:term_status "accepted"@en ;
    skos:definition "Purposes associated with running and management of educational organisations and services"@en ;
    skos:prefLabel "Education Management"@en .

sector-education-owl:ResearchDataManagement a rdfs:Class,
        owl:Class,
        dpv-owl:Purpose ;
    dct:created "2024-12-01"^^xsd:date ;
    rdfs:isDefinedBy sector-education-owl: ;
    rdfs:subClassOf sector-education-owl:ResearchManagement ;
    sw:term_status "accepted"@en ;
    skos:definition "Purposes associated with management of data in an educational or academic research context"@en ;
    skos:prefLabel "Research Data Management"@en .

sector-education-owl:ResearchIntegrityManagement a rdfs:Class,
        owl:Class,
        dpv-owl:Purpose ;
    dct:created "2024-12-01"^^xsd:date ;
    rdfs:isDefinedBy sector-education-owl: ;
    rdfs:subClassOf dpv-owl:OrganisationRiskManagement,
        sector-education-owl:ResearchManagement ;
    sw:term_status "accepted"@en ;
    skos:definition "Purposes associated with assessment, determination, and management of integrity for or of research activities and outputs in an educational or academic research context"@en ;
    skos:prefLabel "Research Integrity Management"@en .

sector-education-owl:ResearchManagement a rdfs:Class,
        owl:Class,
        dpv-owl:Purpose ;
    dct:created "2024-12-01"^^xsd:date ;
    rdfs:isDefinedBy sector-education-owl: ;
    rdfs:subClassOf dpv-owl:AcademicResearch,
        sector-education-owl:EducationManagement ;
    sw:term_status "accepted"@en ;
    skos:definition "Purposes associated with research activities and management of research activities within an educational context e.g. within university departments or research groups"@en ;
    skos:prefLabel "Research Management"@en .

sector-education-owl:ResearchUserStudyManagement a rdfs:Class,
        owl:Class,
        dpv-owl:Purpose ;
    dct:created "2024-12-01"^^xsd:date ;
    rdfs:isDefinedBy sector-education-owl: ;
    rdfs:subClassOf sector-education-owl:ResearchManagement ;
    sw:term_status "accepted"@en ;
    skos:definition "Purposes associated with conducting and assessing studies involving people (as user studies) in an educational or academic research context"@en ;
    skos:prefLabel "Research User Study Management"@en .

sector-education-owl:ServiceProvision a rdfs:Class,
        owl:Class,
        dpv-owl:Purpose ;
    dct:created "2024-12-01"^^xsd:date ;
    rdfs:isDefinedBy sector-education-owl: ;
    rdfs:subClassOf dpv-owl:ServiceProvision,
        sector-education-owl:EducationManagement ;
    sw:term_status "accepted"@en ;
    skos:definition "Purposes associated with provision of educational services, including lectures, seminars, laboratory work, and other similar activities within the context of provision of education"@en ;
    skos:prefLabel "Service Provision"@en .

sector-education-owl:StaffManagement a rdfs:Class,
        owl:Class,
        dpv-owl:Purpose ;
    dct:created "2024-12-01"^^xsd:date ;
    rdfs:isDefinedBy sector-education-owl: ;
    rdfs:subClassOf sector-education-owl:EducationManagement ;
    sw:term_status "accepted"@en ;
    skos:definition "Purposes associated with management of staff and related personnel in educational organisations"@en ;
    skos:prefLabel "Staff Management"@en .

sector-education-owl:StaffPerformanceAssessment a rdfs:Class,
        owl:Class,
        dpv-owl:Purpose ;
    dct:created "2024-12-01"^^xsd:date ;
    rdfs:isDefinedBy sector-education-owl: ;
    rdfs:subClassOf dpv-owl:PersonnelPerformanceMonitoring,
        sector-education-owl:StaffManagement ;
    sw:term_status "accepted"@en ;
    skos:definition "Purposes associated with assessment of performance of staff and related personnel in the context of an educational organisation"@en ;
    skos:prefLabel "Staff Performance Assessment"@en .

sector-education-owl:StudentAcademicPotentialAssessment a rdfs:Class,
        owl:Class,
        dpv-owl:Purpose ;
    dct:created "2024-12-01"^^xsd:date ;
    rdfs:isDefinedBy sector-education-owl: ;
    rdfs:subClassOf sector-education-owl:StudentPerformanceAssessment ;
    sw:term_status "accepted"@en ;
    skos:definition "Purposes associated with assessment of academic potential as a measure of the capability of the student for specific academic or educational courses, programs, or services"@en ;
    skos:prefLabel "Student Academic Potential Assessment"@en .

sector-education-owl:StudentAdmissionManagement a rdfs:Class,
        owl:Class,
        dpv-owl:Purpose ;
    dct:created "2024-12-01"^^xsd:date ;
    rdfs:isDefinedBy sector-education-owl: ;
    rdfs:subClassOf sector-education-owl:AccessManagement,
        sector-education-owl:StudentManagement ;
    sw:term_status "accepted"@en ;
    skos:definition "Purposes associated with management of admission process for current and prospective students"@en ;
    skos:prefLabel "Student Admission Management"@en .

sector-education-owl:StudentAdmissionScreening a rdfs:Class,
        owl:Class,
        dpv-owl:Purpose ;
    dct:created "2024-12-01"^^xsd:date ;
    rdfs:isDefinedBy sector-education-owl: ;
    rdfs:subClassOf sector-education-owl:StudentAdmissionManagement ;
    sw:term_status "accepted"@en ;
    skos:definition "Purposes associated with screening and filtering students and prospective students for the purposes of admission to educational organisations, resources, and services"@en ;
    skos:prefLabel "Student Admission Screening"@en .

sector-education-owl:StudentAllocation a rdfs:Class,
        owl:Class,
        dpv-owl:Purpose ;
    dct:created "2024-12-01"^^xsd:date ;
    rdfs:isDefinedBy sector-education-owl: ;
    rdfs:subClassOf sector-education-owl:StudentManagement ;
    sw:term_status "accepted"@en ;
    skos:definition "Purposes associated with allocation of students to educational institutes, resources, and services"@en ;
    skos:prefLabel "StudentAllocation"@en .

sector-education-owl:StudentAssignmentAssessment a rdfs:Class,
        owl:Class,
        dpv-owl:Purpose ;
    dct:created "2024-12-01"^^xsd:date ;
    rdfs:isDefinedBy sector-education-owl: ;
    rdfs:subClassOf sector-education-owl:StudentLearningOutcomeAssessment ;
    sw:term_status "accepted"@en ;
    skos:definition "Purposes associated with assessment of student performance in the context of an educational assignment or task or other processes where the student is required to perform an activity which is then assessed"@en ;
    skos:prefLabel "Student Assignment Assessment"@en .

sector-education-owl:StudentAttendanceManagement a rdfs:Class,
        owl:Class,
        dpv-owl:Purpose ;
    dct:created "2024-12-01"^^xsd:date ;
    rdfs:isDefinedBy sector-education-owl: ;
    rdfs:subClassOf sector-education-owl:ServiceProvision ;
    sw:term_status "accepted"@en ;
    skos:definition "Purposes associated with undertaking and management of attendance of students within an educational context"@en ;
    skos:prefLabel "Student Attendance Management"@en .

sector-education-owl:StudentCheatingAssessment a rdfs:Class,
        owl:Class,
        dpv-owl:Purpose ;
    dct:created "2024-12-01"^^xsd:date ;
    rdfs:isDefinedBy sector-education-owl: ;
    rdfs:subClassOf dpv-owl:FraudPreventionAndDetection,
        sector-education-owl:StudentIntegrityManagement ;
    sw:term_status "accepted"@en ;
    skos:definition "Purposes associated with detection, assessment, and management of activities considered as cheating or other activities considered to subvert rules or to obtain unfair advantage in the context of educational services and assessments"@en ;
    skos:prefLabel "Student Cheating Assessment"@en .

sector-education-owl:StudentContentDelivery a rdfs:Class,
        owl:Class,
        dpv-owl:Purpose ;
    dct:created "2024-12-01"^^xsd:date ;
    rdfs:isDefinedBy sector-education-owl: ;
    rdfs:subClassOf sector-education-owl:ServiceProvision ;
    sw:term_status "accepted"@en ;
    skos:definition "Purposes associated with delivery of content to student or group of students in the context of educational services"@en ;
    skos:prefLabel "Student Content Delivery"@en .

sector-education-owl:StudentCourseAllocation a rdfs:Class,
        owl:Class,
        dpv-owl:Purpose ;
    dct:created "2024-12-01"^^xsd:date ;
    rdfs:isDefinedBy sector-education-owl: ;
    rdfs:subClassOf sector-education-owl:StudentAllocation ;
    sw:term_status "accepted"@en ;
    skos:definition "Purposes associated with allocation of students to specific courses in the context of educational services"@en ;
    skos:prefLabel "Student Course Allocation"@en .

sector-education-owl:StudentCourseRecommendation a rdfs:Class,
        owl:Class,
        dpv-owl:Purpose ;
    dct:created "2024-12-01"^^xsd:date ;
    rdfs:isDefinedBy sector-education-owl: ;
    rdfs:subClassOf sector-education-owl:StudentAdmissionManagement ;
    sw:term_status "accepted"@en ;
    skos:definition "Purposes associated with providing recommendations to students regarding prospective courses for education"@en ;
    skos:prefLabel "Student Course Recommendation"@en .

sector-education-owl:StudentEligibilityAssessment a rdfs:Class,
        owl:Class,
        dpv-owl:Purpose ;
    dct:created "2024-12-01"^^xsd:date ;
    rdfs:isDefinedBy sector-education-owl: ;
    rdfs:subClassOf sector-education-owl:StudentAdmissionManagement ;
    sw:term_status "accepted"@en ;
    skos:definition "Purposes associated with eligibility assessment of students and prospective students for the purposes of admission and access to educational institutes, resources, and services"@en ;
    skos:prefLabel "Student Eligibility Assessment"@en .

sector-education-owl:StudentEnrollmentManagement a rdfs:Class,
        owl:Class,
        dpv-owl:Purpose ;
    dct:created "2024-12-01"^^xsd:date ;
    rdfs:isDefinedBy sector-education-owl: ;
    rdfs:subClassOf sector-education-owl:StudentAdmissionManagement ;
    sw:term_status "accepted"@en ;
    skos:definition "Purposes associated with enrollement of students and prospective students in educational courses, programs, and institutes"@en ;
    skos:prefLabel "Student Enrollment Management"@en .

sector-education-owl:StudentExamAssessment a rdfs:Class,
        owl:Class,
        dpv-owl:Purpose ;
    dct:created "2024-12-01"^^xsd:date ;
    rdfs:isDefinedBy sector-education-owl: ;
    rdfs:subClassOf sector-education-owl:StudentLearningOutcomeAssessment ;
    sw:term_status "accepted"@en ;
    skos:definition "Purposes associated with assessment of student performance in the context of an educational exam"@en ;
    skos:prefLabel "Student Exam Assessment"@en .

sector-education-owl:StudentFeesManagement a rdfs:Class,
        owl:Class,
        dpv-owl:Purpose ;
    dct:created "2024-12-01"^^xsd:date ;
    rdfs:isDefinedBy sector-education-owl: ;
    rdfs:subClassOf sector-education-owl:StudentAdmissionManagement ;
    sw:term_status "accepted"@en ;
    skos:definition "Purposes associated with management of fees from or for students in the context of educational resources and services"@en ;
    skos:prefLabel "Student Fees Management"@en .

sector-education-owl:StudentFinancialBenefitsManagement a rdfs:Class,
        owl:Class,
        dpv-owl:Purpose ;
    dct:created "2024-12-01"^^xsd:date ;
    rdfs:isDefinedBy sector-education-owl: ;
    rdfs:subClassOf sector-education-owl:StudentAdmissionManagement ;
    sw:term_status "accepted"@en ;
    skos:definition "Purposes associated with management of financial benefits for students in the context of educational resources and services"@en ;
    skos:prefLabel "Student Financial Benefits Management"@en .

sector-education-owl:StudentGuidanceManagement a rdfs:Class,
        owl:Class,
        dpv-owl:Purpose ;
    dct:created "2024-12-01"^^xsd:date ;
    rdfs:isDefinedBy sector-education-owl: ;
    rdfs:subClassOf sector-education-owl:StudentWellbeingManagement ;
    sw:term_status "accepted"@en ;
    skos:definition "Purposes associated with providing and managing guidance, counselling, and other related services within the context of educational services"@en ;
    skos:prefLabel "Student Guidance Management"@en .

sector-education-owl:StudentIdentityVerification a rdfs:Class,
        owl:Class,
        dpv-owl:Purpose ;
    dct:created "2024-12-01"^^xsd:date ;
    rdfs:isDefinedBy sector-education-owl: ;
    rdfs:subClassOf dpv-owl:IdentityVerification,
        sector-education-owl:StudentIntegrityManagement ;
    sw:term_status "accepted"@en ;
    skos:definition "Purposes associated with verification of a student's identity in an educational context, such as for exams or access to resources"@en ;
    skos:prefLabel "Student Identity Verification"@en .

sector-education-owl:StudentInPersonProctoring a rdfs:Class,
        owl:Class,
        dpv-owl:Purpose ;
    dct:created "2024-12-01"^^xsd:date ;
    rdfs:isDefinedBy sector-education-owl: ;
    rdfs:subClassOf sector-education-owl:StudentProctoring ;
    sw:term_status "accepted"@en ;
    skos:definition "Purposes associated with in-person or physical proctoring i.e. monitoring of students physically present within a particular location during an assessment with the aim of ensuring they do not cheat"@en ;
    skos:prefLabel "Student In Person Proctoring"@en .

sector-education-owl:StudentInstituteAllocation a rdfs:Class,
        owl:Class,
        dpv-owl:Purpose ;
    dct:created "2024-12-01"^^xsd:date ;
    rdfs:isDefinedBy sector-education-owl: ;
    rdfs:subClassOf sector-education-owl:StudentAllocation ;
    sw:term_status "accepted"@en ;
    skos:definition "Purposes associated with allocation of students to specific educational or other institutes in the context of educational services"@en ;
    skos:prefLabel "Student Institute Allocation"@en .

sector-education-owl:StudentInstituteRecommendation a rdfs:Class,
        owl:Class,
        dpv-owl:Purpose ;
    dct:created "2024-12-01"^^xsd:date ;
    rdfs:isDefinedBy sector-education-owl: ;
    rdfs:subClassOf sector-education-owl:StudentAdmissionManagement ;
    sw:term_status "accepted"@en ;
    skos:definition "Purposes associated with providing recommendations to students regarding prospective institutes for education"@en ;
    skos:prefLabel "Student Institute Recommendation"@en .

sector-education-owl:StudentIntegrityManagement a rdfs:Class,
        owl:Class,
        dpv-owl:Purpose ;
    dct:created "2024-12-01"^^xsd:date ;
    rdfs:isDefinedBy sector-education-owl: ;
    rdfs:subClassOf dpv-owl:OrganisationRiskManagement,
        sector-education-owl:StudentManagement ;
    sw:term_status "accepted"@en ;
    skos:definition "Purposes associated with integrity assessment and management of students and activities by students in an educational context"@en ;
    skos:prefLabel "Student Integrity Management"@en .

sector-education-owl:StudentIntegrityTraining a rdfs:Class,
        owl:Class,
        dpv-owl:Purpose ;
    dct:created "2024-12-01"^^xsd:date ;
    rdfs:isDefinedBy sector-education-owl: ;
    rdfs:subClassOf sector-education-owl:StudentIntegrityManagement ;
    sw:term_status "accepted"@en ;
    skos:definition "Purposes associated with providing, assessing, and managing training for students regarding integrity in an educational context"@en ;
    skos:prefLabel "Student Integrity Training"@en .

sector-education-owl:StudentLearningFeedbackManagement a rdfs:Class,
        owl:Class,
        dpv-owl:Purpose ;
    dct:created "2024-12-01"^^xsd:date ;
    rdfs:isDefinedBy sector-education-owl: ;
    rdfs:subClassOf sector-education-owl:ServiceProvision ;
    sw:term_status "accepted"@en ;
    skos:definition "Purposes associated with creating, providing, and managing feedback for students regarding their learning potential and outcomes in the context of educational services"@en ;
    skos:prefLabel "Student Learning Feedback Management"@en .

sector-education-owl:StudentLearningNeedsAssessment a rdfs:Class,
        owl:Class,
        dpv-owl:Purpose ;
    dct:created "2024-12-01"^^xsd:date ;
    rdfs:isDefinedBy sector-education-owl: ;
    rdfs:subClassOf sector-education-owl:StudentPerformanceAssessment ;
    sw:term_status "accepted"@en ;
    skos:definition "Purposes associated with assessment of learning needs or a measure of what resources, services, and approaches are needed for a student to learn and gain specific knowledge or group of knowledge within an educational context"@en ;
    skos:prefLabel "Student Learning Needs Assessment"@en .

sector-education-owl:StudentLearningOutcomeAssessment a rdfs:Class,
        owl:Class,
        dpv-owl:Purpose ;
    dct:created "2024-12-01"^^xsd:date ;
    rdfs:isDefinedBy sector-education-owl: ;
    rdfs:subClassOf sector-education-owl:StudentPerformanceAssessment ;
    sw:term_status "accepted"@en ;
    skos:definition "Purposes associated with assessment of student performance in the context of meeting learning outcomes as set within the educational course or program"@en ;
    skos:prefLabel "Student Learning Outcome Assessment"@en .

sector-education-owl:StudentManagement a rdfs:Class,
        owl:Class,
        dpv-owl:Purpose ;
    dct:created "2024-12-01"^^xsd:date ;
    rdfs:isDefinedBy sector-education-owl: ;
    rdfs:subClassOf sector-education-owl:EducationManagement ;
    sw:term_status "accepted"@en ;
    skos:definition "Purposes associated with management of current and prospective students"@en ;
    skos:prefLabel "Student Management"@en .

sector-education-owl:StudentMisconductInvestigation a rdfs:Class,
        owl:Class,
        dpv-owl:Purpose ;
    dct:created "2024-12-01"^^xsd:date ;
    rdfs:isDefinedBy sector-education-owl: ;
    rdfs:subClassOf sector-education-owl:StudentIntegrityManagement ;
    sw:term_status "accepted"@en ;
    skos:definition "Purposes associated with investigating and assessing potential misconduct by or on a student or a group of students in an educational context"@en ;
    skos:prefLabel "Student Misconduct Investigation"@en .

sector-education-owl:StudentOnlineProctoring a rdfs:Class,
        owl:Class,
        dpv-owl:Purpose ;
    dct:created "2024-12-01"^^xsd:date ;
    rdfs:isDefinedBy sector-education-owl: ;
    rdfs:subClassOf sector-education-owl:StudentProctoring ;
    sw:term_status "accepted"@en ;
    skos:definition "Purposes associated with online or virtual or remote proctoring i.e. monitoring of students present virtually over an online platform or within their remote physical location during an assessment with the aim of ensuring they do not cheat"@en ;
    skos:prefLabel "Student Online Proctoring"@en .

sector-education-owl:StudentPerformanceAssessment a rdfs:Class,
        owl:Class,
        dpv-owl:Purpose ;
    dct:created "2024-12-01"^^xsd:date ;
    rdfs:isDefinedBy sector-education-owl: ;
    rdfs:subClassOf sector-education-owl:StudentManagement ;
    sw:term_status "accepted"@en ;
    skos:definition "Purposes associated with assessment of student performance, including through exams and assignments, in educational contexts"@en ;
    skos:prefLabel "Student Performance Assessment"@en .

sector-education-owl:StudentPerformanceManagement a rdfs:Class,
        owl:Class,
        dpv-owl:Purpose ;
    dct:created "2024-12-01"^^xsd:date ;
    rdfs:isDefinedBy sector-education-owl: ;
    rdfs:subClassOf sector-education-owl:StudentManagement ;
    sw:term_status "accepted"@en ;
    skos:definition "Purposes associated with management of student performance in educational contexts"@en ;
    skos:prefLabel "Student Performance Management"@en .

sector-education-owl:StudentPerformanceMonitoring a rdfs:Class,
        owl:Class,
        dpv-owl:Purpose ;
    dct:created "2024-12-01"^^xsd:date ;
    rdfs:isDefinedBy sector-education-owl: ;
    rdfs:subClassOf sector-education-owl:StudentManagement ;
    sw:term_status "accepted"@en ;
    skos:definition "Purposes associated with monitoring of student performance in educational contexts"@en ;
    skos:prefLabel "Student Performance Monitoring"@en .

sector-education-owl:StudentPersonalisedContentDelivery a rdfs:Class,
        owl:Class,
        dpv-owl:Purpose ;
    dct:created "2024-12-01"^^xsd:date ;
    rdfs:isDefinedBy sector-education-owl: ;
    rdfs:subClassOf dpv-owl:Personalisation,
        sector-education-owl:ServiceProvision ;
    sw:term_status "accepted"@en ;
    skos:definition "Purposes associated with personalisation of the content delivery for an individual student or a group of students in the context of educational services"@en ;
    skos:prefLabel "Student Personalised Content Delivery"@en .

sector-education-owl:StudentPlagiarismDetection a rdfs:Class,
        owl:Class,
        dpv-owl:Purpose ;
    dct:created "2024-12-01"^^xsd:date ;
    rdfs:isDefinedBy sector-education-owl: ;
    rdfs:subClassOf dpv-owl:FraudPreventionAndDetection,
        sector-education-owl:StudentIntegrityManagement ;
    sw:term_status "accepted"@en ;
    skos:definition "Purposes associated with determination of plagiarism demonstrated by a student or students or present within the work submitted by a student or students in an educational context"@en ;
    skos:prefLabel "Student Plagiarism Detection"@en .

sector-education-owl:StudentProctoring a rdfs:Class,
        owl:Class,
        dpv-owl:Purpose ;
    dct:created "2024-12-01"^^xsd:date ;
    rdfs:isDefinedBy sector-education-owl: ;
    rdfs:subClassOf sector-education-owl:StudentCheatingAssessment ;
    sw:term_status "accepted"@en ;
    skos:definition "Purposes associated with proctoring i.e. monitoring of students during an assessment with the aim of ensuring they do not cheat"@en ;
    skos:prefLabel "Student Proctoring"@en .

sector-education-owl:StudentProgramAllocation a rdfs:Class,
        owl:Class,
        dpv-owl:Purpose ;
    dct:created "2024-12-01"^^xsd:date ;
    rdfs:isDefinedBy sector-education-owl: ;
    rdfs:subClassOf sector-education-owl:StudentAllocation ;
    sw:term_status "accepted"@en ;
    skos:definition "Purposes associated with allocation of students to specific programs in the context of educational services"@en ;
    skos:prefLabel "Student Program Allocation"@en .

sector-education-owl:StudentProgramRecommendation a rdfs:Class,
        owl:Class,
        dpv-owl:Purpose ;
    dct:created "2024-12-01"^^xsd:date ;
    rdfs:isDefinedBy sector-education-owl: ;
    rdfs:subClassOf sector-education-owl:StudentAdmissionManagement ;
    sw:term_status "accepted"@en ;
    skos:definition "Purposes associated with providing recommendations to students regarding prospective programs for education"@en ;
    skos:prefLabel "Student Program Recommendation"@en .

sector-education-owl:StudentResourceAccessManagement a rdfs:Class,
        owl:Class,
        dpv-owl:Purpose ;
    dct:created "2024-12-01"^^xsd:date ;
    rdfs:isDefinedBy sector-education-owl: ;
    rdfs:subClassOf sector-education-owl:ServiceProvision ;
    sw:term_status "accepted"@en ;
    skos:definition "Purposes associated with determining and managing access to students to specific resources within an educational context, such as laboratory equipment or library resources"@en ;
    skos:prefLabel "Student Resource Access Management"@en .

sector-education-owl:StudentSocialActivitiesManagement a rdfs:Class,
        owl:Class,
        dpv-owl:Purpose ;
    dct:created "2024-12-01"^^xsd:date ;
    rdfs:isDefinedBy sector-education-owl: ;
    rdfs:subClassOf sector-education-owl:StudentManagement ;
    sw:term_status "accepted"@en ;
    skos:definition "Purposes associated with promotion, admission, and management of social activities for students within an educational context"@en ;
    skos:prefLabel "Student Social Activities Management"@en .

sector-education-owl:StudentSpecialNeedsManagement a rdfs:Class,
        owl:Class,
        dpv-owl:Purpose ;
    dct:created "2024-12-01"^^xsd:date ;
    rdfs:isDefinedBy sector-education-owl: ;
    rdfs:subClassOf sector-education-owl:StudentAdmissionManagement ;
    sw:term_status "accepted"@en ;
    skos:definition "Purposes associated with determination and management of special needs of students and prospective students in the context of educational services and resources"@en ;
    skos:prefLabel "Student Special Needs Management"@en .

sector-education-owl:StudentWellbeingManagement a rdfs:Class,
        owl:Class,
        dpv-owl:Purpose ;
    dct:created "2024-12-01"^^xsd:date ;
    rdfs:isDefinedBy sector-education-owl: ;
    rdfs:subClassOf sector-education-owl:StudentManagement ;
    sw:term_status "accepted"@en ;
    skos:definition "Purposes associated with management of student wellbeing in an educational context"@en ;
    skos:prefLabel "Student Wellbeing Management"@en .

sector-education-owl:serialisation-html a profile:ResourceDescriptor ;
    dct:conformsTo <https://www.w3.org/TR/html/> ;
    dct:format <https://www.iana.org/assignments/media-types/text/html> ;
    dct:title "Education Sector Concepts - HTML serialiation" ;
    profile:hasArtifact <https://w3id.org/dpv/sector/education/sector-education-owl.html> ;
    profile:hasRole role:specification .

sector-education-owl:serialisation-jsonld a profile:ResourceDescriptor ;
    dct:conformsTo <https://www.w3.org/TR/json-ld11/> ;
    dct:format <https://www.iana.org/assignments/media-types/application/ld+json> ;
    dct:title "Education Sector Concepts - JSON-LD serialiation" ;
    profile:hasArtifact <https://w3id.org/dpv/sector/education/sector-education-owl.jsonld> ;
    profile:hasRole role:vocabulary .

sector-education-owl:serialisation-n3 a profile:ResourceDescriptor ;
    dct:conformsTo <https://www.w3.org/TeamSubmission/n3/> ;
    dct:format <https://www.iana.org/assignments/media-types/text/n3> ;
    dct:title "Education Sector Concepts - N3 serialiation" ;
    profile:hasArtifact <https://w3id.org/dpv/sector/education/sector-education-owl.n3> ;
    profile:hasRole role:vocabulary .

sector-education-owl:serialisation-rdf a profile:ResourceDescriptor ;
    dct:conformsTo rdf: ;
    dct:format <https://www.iana.org/assignments/media-types/application/rdf+xml> ;
    dct:title "Education Sector Concepts - RDF/XML serialiation" ;
    profile:hasArtifact <https://w3id.org/dpv/sector/education/sector-education-owl.rdf> ;
    profile:hasRole role:vocabulary .

sector-education-owl:serialisation-ttl a profile:ResourceDescriptor ;
    dct:conformsTo <https://www.w3.org/TR/turtle/> ;
    dct:format <https://www.iana.org/assignments/media-types/text/turtle> ;
    dct:title "Education Sector Concepts - Turtle serialiation" ;
    profile:hasArtifact <https://w3id.org/dpv/sector/education/sector-education-owl.ttl> ;
    profile:hasRole role:vocabulary .

<https://w3id.org/dpv/examples> a profile:ResourceDescriptor ;
    dct:conformsTo <https://www.w3.org/TR/html/> ;
    dct:format <https://www.iana.org/assignments/media-types/text/html> ;
    dct:title "Examples for Data Privacy Vocabulary" ;
    profile:hasArtifact <https://w3id.org/dpv/examples> ;
    profile:hasRole role:guidance .

<https://w3id.org/dpv/guides> a profile:ResourceDescriptor ;
    dct:conformsTo <https://www.w3.org/TR/html/> ;
    dct:format <https://www.iana.org/assignments/media-types/text/html> ;
    dct:title "Guides for Data Privacy Vocabulary" ;
    profile:hasArtifact <https://w3id.org/dpv/guides> ;
    profile:hasRole role:guidance .

<https://w3id.org/dpv/primer> a profile:ResourceDescriptor ;
    dct:conformsTo <https://www.w3.org/TR/html/> ;
    dct:format <https://www.iana.org/assignments/media-types/text/html> ;
    dct:title "Primer for Data Privacy Vocabulary" ;
    profile:hasArtifact <https://w3id.org/dpv/primer> ;
    profile:hasRole role:guidance .

sector-education-owl: a owl:Ontology,
        profile:Profile ;
    dct:bibliographicCitation "Harshvardhan J. Pandit, Beatriz Esteves, Georg P. Krog, Paul Ryan, Delaram Golpayegani, Julian Flake (2025) Data Privacy Vocabulary (DPV) – Version 2.0. In: Demartini, G., et al. The Semantic Web – ISWC 2024. ISWC 2024. Lecture Notes in Computer Science, vol 15233. Springer, Cham. https://doi.org/10.1007/978-3-031-77847-6_10" ;
    dct:conformsTo <http://www.w3.org/2002/07/owl>,
        "http://www.w3.org/2000/01/rdf-schema",
        "http://www.w3.org/2004/02/skos/core" ;
    dct:created "2024-12-01"@en ;
    dct:creator [ a dct:Agent,
                foaf:Person ;
            scoro:hasORCID "0000-0002-5068-3714" ;
            org:memberOf [ a foaf:Organization ;
                    foaf:name "ADAPT Centre, Dublin City University" ] ;
            foaf:homepage "https://harshp.com/" ;
            foaf:name "Harshvardhan J. Pandit" ] ;
    dct:description "Extension to the Data Privacy Vocabulary (DPV) providing concepts for the education sector"@en ;
    dct:hasVersion sector-education-owl: ;
    dct:identifier "https://w3id.org/dpv/sector/education" ;
    dct:issued "2024-12-01"@en ;
    dct:license <https://www.w3.org/copyright/document-license-2023/> ;
    dct:modified "2025-03-16"@en ;
    dct:publisher <https://www.w3.org/> ;
    dct:source <https://www.w3.org/groups/cg/dpvcg/> ;
    dct:title "Education Sector Concepts"@en ;
    bibo:doi "10.5281/zenodo.12505841" ;
    bibo:status "http://purl.org/ontology/bibo/status/draft" ;
    vann:preferredNamespacePrefix "sector-education" ;
    vann:preferredNamespaceUri "https://w3id.org/dpv/sector/education#" ;
    rdfs:Label "SECTOR-EDUCATION"@en ;
    owl:versionIRI <https://w3id.org/dpv/2.1/sector/education/owl#> ;
    owl:versionInfo "2.1" ;
    profile:hasResource <https://w3id.org/dpv/examples>,
        <https://w3id.org/dpv/guides>,
        <https://w3id.org/dpv/primer>,
        sector-education-owl:serialisation-html,
        sector-education-owl:serialisation-jsonld,
        sector-education-owl:serialisation-n3,
        sector-education-owl:serialisation-rdf,
        sector-education-owl:serialisation-ttl ;
    profile:isProfileOf <http://www.w3.org/2002/07/owl>,
        <https://w3id.org/dpv/owl>,
        sector-education-owl: ;
    foaf:logo <https://w3id.org/dpv/media/logo.png> ;
    schema:version "2.1" .

