@prefix bibo: <http://purl.org/ontology/bibo/> .
@prefix dcam: <http://purl.org/dc/dcam/> .
@prefix dct: <http://purl.org/dc/terms/> .
@prefix dpv: <https://w3id.org/dpv#> .
@prefix foaf: <http://xmlns.com/foaf/0.1/> .
@prefix org: <http://www.w3.org/ns/org#> .
@prefix owl: <http://www.w3.org/2002/07/owl#> .
@prefix profile: <http://www.w3.org/ns/dx/prof/> .
@prefix rdf: <http://www.w3.org/1999/02/22-rdf-syntax-ns#> .
@prefix rdfs: <http://www.w3.org/2000/01/rdf-schema#> .
@prefix role: <http://www.w3.org/ns/dx/prof/role/> .
@prefix schema: <https://schema.org/> .
@prefix scoro: <http://purl.org/spar/scoro/> .
@prefix skos: <http://www.w3.org/2004/02/skos/core#> .
@prefix sw: <http://www.w3.org/2003/06/sw-vocab-status/ns#> .
@prefix tech: <https://w3id.org/dpv/tech#> .
@prefix vann: <http://purl.org/vocab/vann/> .
@prefix xsd: <http://www.w3.org/2001/XMLSchema#> .

tech:API a rdfs:Class,
        skos:Concept,
        dpv:Technology ;
    dct:contributor _:N0a43dd9ea5e94fe695d8b7df8802cfdd,
        _:Ne8d6151e3d8047e6a947b3ec1a3830a1 ;
    dct:created "2024-12-01"^^xsd:date ;
    rdfs:isDefinedBy tech: ;
    sw:term_status "accepted"@en ;
    skos:broader tech:Algorithm ;
    skos:definition "A set of rules and protocols to communicate and exchange data between applications"@en ;
    skos:inScheme tech:tools-classes ;
    skos:prefLabel "API"@en .

tech:Algorithm a rdfs:Class,
        skos:Concept,
        dpv:Technology ;
    dct:contributor _:N0a43dd9ea5e94fe695d8b7df8802cfdd,
        _:Ne8d6151e3d8047e6a947b3ec1a3830a1 ;
    dct:created "2024-12-01"^^xsd:date ;
    rdfs:isDefinedBy tech: ;
    sw:term_status "accepted"@en ;
    skos:broader dpv:Technology ;
    skos:definition "A step-by-step set of instructions used to solve a problem or perform a computation"@en ;
    skos:inScheme tech:tools-classes ;
    skos:prefLabel "Algorithm"@en .

tech:Android a rdfs:Class,
        skos:Concept,
        dpv:Technology ;
    dct:contributor _:N0a43dd9ea5e94fe695d8b7df8802cfdd ;
    dct:created "2022-06-15"^^xsd:date ;
    rdfs:isDefinedBy tech: ;
    sw:term_status "accepted"@en ;
    skos:broader tech:OS ;
    skos:definition "Android operating system"@en ;
    skos:inScheme tech:tools-classes ;
    skos:prefLabel "Android"@en .

tech:AppStore a rdfs:Class,
        skos:Concept,
        dpv:Technology ;
    dct:contributor _:N0a43dd9ea5e94fe695d8b7df8802cfdd ;
    dct:created "2022-06-15"^^xsd:date ;
    rdfs:isDefinedBy tech: ;
    sw:term_status "accepted"@en ;
    skos:broader tech:Application ;
    skos:definition "An application or platform for distribution of other applications"@en ;
    skos:inScheme tech:tools-classes ;
    skos:prefLabel "Application Store"@en .

tech:Application a rdfs:Class,
        skos:Concept,
        dpv:Technology ;
    dct:contributor _:N0a43dd9ea5e94fe695d8b7df8802cfdd ;
    dct:created "2022-06-15"^^xsd:date ;
    rdfs:isDefinedBy tech: ;
    sw:term_status "accepted"@en ;
    skos:broader tech:Software ;
    skos:definition "Application or Application Software"@en ;
    skos:inScheme tech:tools-classes ;
    skos:prefLabel "Application"@en .

tech:ApplicationSpecificIntegratedCircuit a rdfs:Class,
        skos:Concept,
        dpv:Technology ;
    dct:contributor _:N0a43dd9ea5e94fe695d8b7df8802cfdd,
        _:Ne8d6151e3d8047e6a947b3ec1a3830a1 ;
    dct:created "2024-12-01"^^xsd:date ;
    rdfs:isDefinedBy tech: ;
    sw:term_status "accepted"@en ;
    skos:broader tech:IntegratedCircuit ;
    skos:definition "A custom-designed integrated circuit optimised for a specific task"@en ;
    skos:inScheme tech:tools-classes ;
    skos:prefLabel "ApplicationSpecificIntegratedCircuit"@en .

tech:CloudService a rdfs:Class,
        skos:Concept,
        dpv:Technology ;
    dct:contributor _:N0a43dd9ea5e94fe695d8b7df8802cfdd ;
    dct:created "2024-12-01"^^xsd:date ;
    rdfs:isDefinedBy tech: ;
    sw:term_status "accepted"@en ;
    skos:broader dpv:Technology ;
    skos:definition "A remotely accessible service delivered over the internet for providing resources, software, or infrastructure"@en ;
    skos:inScheme tech:tools-classes ;
    skos:prefLabel "Cloud Service Provision"@en .

tech:CloudStorage a rdfs:Class,
        skos:Concept,
        dpv:Technology ;
    dct:contributor _:N0a43dd9ea5e94fe695d8b7df8802cfdd ;
    dct:created "2022-06-15"^^xsd:date ;
    rdfs:isDefinedBy tech: ;
    sw:term_status "accepted"@en ;
    skos:broader tech:DataStorage ;
    skos:definition "Storage utilising cloud technologies"@en ;
    skos:inScheme tech:tools-classes ;
    skos:prefLabel "Cloud Storage"@en .

tech:Component a rdfs:Class,
        skos:Concept,
        dpv:Technology ;
    dct:contributor _:N0a43dd9ea5e94fe695d8b7df8802cfdd,
        _:Ne8d6151e3d8047e6a947b3ec1a3830a1 ;
    dct:created "2024-12-01"^^xsd:date ;
    rdfs:isDefinedBy tech: ;
    sw:term_status "accepted"@en ;
    skos:broader dpv:Technology ;
    skos:definition "A self-contained part of a system that performs a specific function and interacts with other components"@en ;
    skos:inScheme tech:tools-classes ;
    skos:prefLabel "Component"@en .

tech:Cookie a rdfs:Class,
        skos:Concept,
        dpv:Technology ;
    dct:contributor _:N0a43dd9ea5e94fe695d8b7df8802cfdd ;
    dct:created "2022-06-15"^^xsd:date ;
    rdfs:isDefinedBy tech: ;
    sw:term_status "accepted"@en ;
    skos:broader tech:LocalStorage ;
    skos:definition "A HTTP or web or internet cookie"@en ;
    skos:inScheme tech:tools-classes ;
    skos:prefLabel "Cookie"@en .

tech:DataStorage a rdfs:Class,
        skos:Concept,
        dpv:Technology ;
    dct:contributor _:N0a43dd9ea5e94fe695d8b7df8802cfdd ;
    dct:created "2022-06-15"^^xsd:date ;
    rdfs:isDefinedBy tech: ;
    sw:term_status "accepted"@en ;
    skos:broader tech:Software ;
    skos:definition "Technology associated with storage of data"@en ;
    skos:inScheme tech:tools-classes ;
    skos:prefLabel "Data Storage"@en .

tech:Database a rdfs:Class,
        skos:Concept,
        dpv:Technology ;
    dct:contributor _:N0a43dd9ea5e94fe695d8b7df8802cfdd ;
    dct:created "2022-06-15"^^xsd:date ;
    rdfs:isDefinedBy tech: ;
    sw:term_status "accepted"@en ;
    skos:broader tech:DataStorage ;
    skos:definition "A database, database management system (DBMS), or application database"@en ;
    skos:inScheme tech:tools-classes ;
    skos:prefLabel "Database"@en .

tech:DesktopPC a rdfs:Class,
        skos:Concept,
        dpv:Technology ;
    dct:contributor _:N0a43dd9ea5e94fe695d8b7df8802cfdd ;
    dct:created "2022-06-15"^^xsd:date ;
    rdfs:isDefinedBy tech: ;
    sw:term_status "accepted"@en ;
    skos:broader tech:PersonalComputer ;
    skos:definition "A non-portable or fixed personal computer"@en ;
    skos:inScheme tech:tools-classes ;
    skos:prefLabel "Desktop PC"@en .

tech:Device a rdfs:Class,
        skos:Concept,
        dpv:Technology ;
    dct:contributor _:N0a43dd9ea5e94fe695d8b7df8802cfdd ;
    dct:created "2022-06-15"^^xsd:date ;
    rdfs:isDefinedBy tech: ;
    sw:term_status "accepted"@en ;
    skos:broader tech:Hardware ;
    skos:definition "Device or computing device"@en ;
    skos:inScheme tech:tools-classes ;
    skos:prefLabel "Device"@en .

tech:GNULinux a rdfs:Class,
        skos:Concept,
        dpv:Technology ;
    dct:contributor _:N0a43dd9ea5e94fe695d8b7df8802cfdd ;
    dct:created "2022-06-15"^^xsd:date ;
    rdfs:isDefinedBy tech: ;
    sw:term_status "accepted"@en ;
    skos:broader tech:OS ;
    skos:definition "GNU/Linux operating system"@en ;
    skos:inScheme tech:tools-classes ;
    skos:prefLabel "GNU/Linux"@en .

tech:Hardware a rdfs:Class,
        skos:Concept,
        dpv:Technology ;
    dct:contributor _:N0a43dd9ea5e94fe695d8b7df8802cfdd ;
    dct:created "2022-06-15"^^xsd:date ;
    rdfs:isDefinedBy tech: ;
    sw:term_status "accepted"@en ;
    skos:broader dpv:Technology ;
    skos:definition "Physical parts or components of the technology"@en ;
    skos:inScheme tech:tools-classes ;
    skos:prefLabel "Hardware"@en .

tech:Infrastructure a rdfs:Class,
        skos:Concept,
        dpv:Technology ;
    dct:contributor _:N0a43dd9ea5e94fe695d8b7df8802cfdd,
        _:Ne8d6151e3d8047e6a947b3ec1a3830a1 ;
    dct:created "2024-12-01"^^xsd:date ;
    rdfs:isDefinedBy tech: ;
    sw:term_status "accepted"@en ;
    skos:broader dpv:Technology ;
    skos:definition "The foundational hardware, software, and other resources to support the operation of systems or services"@en ;
    skos:inScheme tech:tools-classes ;
    skos:prefLabel "Infrastructure as a Service (IaaS) Provision"@en .

tech:IntegratedCircuit a rdfs:Class,
        skos:Concept,
        dpv:Technology ;
    dct:contributor _:N0a43dd9ea5e94fe695d8b7df8802cfdd,
        _:Ne8d6151e3d8047e6a947b3ec1a3830a1 ;
    dct:created "2024-12-01"^^xsd:date ;
    rdfs:isDefinedBy tech: ;
    sw:term_status "accepted"@en ;
    skos:broader tech:Hardware ;
    skos:definition "A integrated electronic chip containing interconnected components to perform specific functions"@en ;
    skos:inScheme tech:tools-classes ;
    skos:prefLabel "IntegratedCircuit"@en .

tech:IoT a rdfs:Class,
        skos:Concept,
        dpv:Technology ;
    dct:contributor _:N0a43dd9ea5e94fe695d8b7df8802cfdd,
        _:Ne8d6151e3d8047e6a947b3ec1a3830a1 ;
    dct:created "2024-12-01"^^xsd:date ;
    dct:source "ISO/IEC 22989:2022"@en ;
    rdfs:isDefinedBy tech: ;
    sw:term_status "accepted"@en ;
    skos:broader tech:Hardware ;
    skos:definition "IoT is the infrastructure of interconnected entities, people, systems and information resources together with services that process and react to information from the physical world and virtual world"@en ;
    skos:inScheme tech:tools-classes ;
    skos:prefLabel "Internet of Things (IoT)"@en .

tech:IoTDevice a rdfs:Class,
        skos:Concept,
        dpv:Technology ;
    dct:contributor _:N0a43dd9ea5e94fe695d8b7df8802cfdd,
        _:Ne8d6151e3d8047e6a947b3ec1a3830a1 ;
    dct:created "2024-12-01"^^xsd:date ;
    dct:source "ISO/IEC 22989:2022"@en ;
    rdfs:isDefinedBy tech: ;
    sw:term_status "accepted"@en ;
    skos:broader tech:Device,
        tech:IoT ;
    skos:definition "An entity of an IoT system that interacts and communicates with the physical world through sensing or actuating"@en ;
    skos:inScheme tech:tools-classes ;
    skos:prefLabel "IoT Device"@en .

tech:IoTSystem a rdfs:Class,
        skos:Concept,
        dpv:Technology ;
    dct:contributor _:N0a43dd9ea5e94fe695d8b7df8802cfdd,
        _:Ne8d6151e3d8047e6a947b3ec1a3830a1 ;
    dct:created "2024-12-01"^^xsd:date ;
    dct:source "ISO/IEC 22989:2022"@en ;
    rdfs:isDefinedBy tech: ;
    sw:term_status "accepted"@en ;
    skos:broader tech:IoT,
        tech:System ;
    skos:definition "A specific system that is an implementation or application of the IoT framework and contains interconnected IoT devices and their communication network along with other hardware and software required for providing functionalities"@en ;
    skos:inScheme tech:tools-classes ;
    skos:prefLabel "IoT System"@en .

tech:LaptopPC a rdfs:Class,
        skos:Concept,
        dpv:Technology ;
    dct:contributor _:N0a43dd9ea5e94fe695d8b7df8802cfdd ;
    dct:created "2022-06-15"^^xsd:date ;
    rdfs:isDefinedBy tech: ;
    sw:term_status "accepted"@en ;
    skos:broader tech:PersonalComputer ;
    skos:definition "A portal personal computer"@en ;
    skos:inScheme tech:tools-classes ;
    skos:prefLabel "Laptop PC"@en .

tech:LocalStorage a rdfs:Class,
        skos:Concept,
        dpv:Technology ;
    dct:contributor _:N0a43dd9ea5e94fe695d8b7df8802cfdd ;
    dct:created "2022-06-15"^^xsd:date ;
    rdfs:isDefinedBy tech: ;
    sw:term_status "accepted"@en ;
    skos:broader tech:DataStorage ;
    skos:definition "Storage that is local (e.g. on device)"@en ;
    skos:inScheme tech:tools-classes ;
    skos:prefLabel "Local Storage"@en .

tech:MSWindows a rdfs:Class,
        skos:Concept,
        dpv:Technology ;
    dct:contributor _:N0a43dd9ea5e94fe695d8b7df8802cfdd ;
    dct:created "2022-06-15"^^xsd:date ;
    rdfs:isDefinedBy tech: ;
    sw:term_status "accepted"@en ;
    skos:broader tech:OS ;
    skos:definition "Microsoft Windows operating system"@en ;
    skos:inScheme tech:tools-classes ;
    skos:prefLabel "Microsoft Windows"@en .

tech:MobilePhone a rdfs:Class,
        skos:Concept,
        dpv:Technology ;
    dct:contributor _:N0a43dd9ea5e94fe695d8b7df8802cfdd ;
    dct:created "2022-06-15"^^xsd:date ;
    rdfs:isDefinedBy tech: ;
    sw:term_status "accepted"@en ;
    skos:broader tech:Telephone ;
    skos:definition "Mobile telephone"@en ;
    skos:inScheme tech:tools-classes ;
    skos:prefLabel "Mobile Phone"@en .

tech:Model a rdfs:Class,
        skos:Concept,
        dpv:Technology ;
    dct:contributor _:N0a43dd9ea5e94fe695d8b7df8802cfdd,
        _:Ne8d6151e3d8047e6a947b3ec1a3830a1 ;
    dct:created "2024-12-01"^^xsd:date ;
    rdfs:isDefinedBy tech: ;
    sw:term_status "accepted"@en ;
    skos:broader dpv:Technology ;
    skos:definition "A simplified representation or abstraction of a system, process, or concept"@en ;
    skos:inScheme tech:tools-classes ;
    skos:prefLabel "Model"@en .

tech:OS a rdfs:Class,
        skos:Concept,
        dpv:Technology ;
    dct:contributor _:N0a43dd9ea5e94fe695d8b7df8802cfdd ;
    dct:created "2022-06-15"^^xsd:date ;
    rdfs:isDefinedBy tech: ;
    sw:term_status "accepted"@en ;
    skos:broader tech:Software ;
    skos:definition "Software for managing hardware and other software"@en ;
    skos:inScheme tech:tools-classes ;
    skos:prefLabel "Operating System (OS)"@en .

tech:PersonalComputer a rdfs:Class,
        skos:Concept,
        dpv:Technology ;
    dct:contributor _:N0a43dd9ea5e94fe695d8b7df8802cfdd ;
    dct:created "2022-06-15"^^xsd:date ;
    rdfs:isDefinedBy tech: ;
    sw:term_status "accepted"@en ;
    skos:broader tech:Device ;
    skos:definition "A computing device intended for individual use"@en ;
    skos:inScheme tech:tools-classes ;
    skos:prefLabel "Personal Computer (PC)"@en .

tech:Platform a rdfs:Class,
        skos:Concept,
        dpv:Technology ;
    dct:contributor _:N0a43dd9ea5e94fe695d8b7df8802cfdd,
        _:Ne8d6151e3d8047e6a947b3ec1a3830a1 ;
    dct:created "2024-12-01"^^xsd:date ;
    rdfs:isDefinedBy tech: ;
    sw:term_status "accepted"@en ;
    skos:broader dpv:Technology ;
    skos:definition "A digital environment that provides tools, infrastructure, and services for developing, deploying, and running applications"@en ;
    skos:inScheme tech:tools-classes ;
    skos:prefLabel "Platform"@en .

tech:Service a rdfs:Class,
        skos:Concept,
        dpv:Technology ;
    dct:contributor _:N0a43dd9ea5e94fe695d8b7df8802cfdd ;
    dct:created "2024-12-01"^^xsd:date ;
    rdfs:isDefinedBy tech: ;
    sw:term_status "accepted"@en ;
    skos:broader dpv:Technology ;
    skos:definition "The carrying out of a specific task or set of tasks as a service"@en ;
    skos:inScheme tech:tools-classes ;
    skos:prefLabel "Service"@en ;
    skos:scopeNote "This concept is distinct from dpv:Service as it represents the notion of a technical service whereas dpv:Service can also refer to organisational, legal, social, and other meanings of service"@en .

tech:Smartphone a rdfs:Class,
        skos:Concept,
        dpv:Technology ;
    dct:contributor _:N0a43dd9ea5e94fe695d8b7df8802cfdd ;
    dct:created "2022-06-15"^^xsd:date ;
    rdfs:isDefinedBy tech: ;
    sw:term_status "accepted"@en ;
    skos:broader tech:MobilePhone,
        tech:PersonalComputer ;
    skos:definition "A combination of a mobile phone with computing capabilities similar to a PC"@en ;
    skos:inScheme tech:tools-classes ;
    skos:prefLabel "Smartphone"@en .

tech:SmartphoneApplication a rdfs:Class,
        skos:Concept,
        dpv:Technology ;
    dct:contributor _:N0a43dd9ea5e94fe695d8b7df8802cfdd ;
    dct:created "2022-06-15"^^xsd:date ;
    rdfs:isDefinedBy tech: ;
    sw:term_status "accepted"@en ;
    skos:broader tech:Application ;
    skos:definition "A computing or digital program on a smartphone device"@en ;
    skos:inScheme tech:tools-classes ;
    skos:prefLabel "Smartphone Application"@en .

tech:Software a rdfs:Class,
        skos:Concept,
        dpv:Technology ;
    dct:contributor _:N0a43dd9ea5e94fe695d8b7df8802cfdd ;
    dct:created "2022-06-15"^^xsd:date ;
    rdfs:isDefinedBy tech: ;
    sw:term_status "accepted"@en ;
    skos:broader dpv:Technology ;
    skos:definition "Virtual parts or components of the technology such as programs and data"@en ;
    skos:inScheme tech:tools-classes ;
    skos:prefLabel "Software"@en .

tech:SoftwareFramework a rdfs:Class,
        skos:Concept,
        dpv:Technology ;
    dct:contributor _:N0a43dd9ea5e94fe695d8b7df8802cfdd,
        _:Ne8d6151e3d8047e6a947b3ec1a3830a1 ;
    dct:created "2024-12-01"^^xsd:date ;
    rdfs:isDefinedBy tech: ;
    sw:term_status "accepted"@en ;
    skos:broader tech:Software ;
    skos:definition "An opinionated collection of functions and architecture design choices for building applications"@en ;
    skos:inScheme tech:tools-classes ;
    skos:prefLabel "SoftwareFramework"@en .

tech:SoftwareLibrary a rdfs:Class,
        skos:Concept,
        dpv:Technology ;
    dct:contributor _:N0a43dd9ea5e94fe695d8b7df8802cfdd,
        _:Ne8d6151e3d8047e6a947b3ec1a3830a1 ;
    dct:created "2024-12-01"^^xsd:date ;
    rdfs:isDefinedBy tech: ;
    sw:term_status "accepted"@en ;
    skos:broader tech:Software ;
    skos:definition "A collection of pre-built and reusable functions for use in development and management of software"@en ;
    skos:inScheme tech:tools-classes ;
    skos:prefLabel "SoftwareLibrary"@en .

tech:System a rdfs:Class,
        skos:Concept,
        dpv:Technology ;
    dct:contributor _:N0a43dd9ea5e94fe695d8b7df8802cfdd,
        _:Ne8d6151e3d8047e6a947b3ec1a3830a1 ;
    dct:created "2024-12-01"^^xsd:date ;
    rdfs:isDefinedBy tech: ;
    sw:term_status "accepted"@en ;
    skos:broader dpv:Technology ;
    skos:definition "A collection of components that interact to achieve a specific goal or function"@en ;
    skos:inScheme tech:tools-classes ;
    skos:prefLabel "System"@en .

tech:Telephone a rdfs:Class,
        skos:Concept,
        dpv:Technology ;
    dct:contributor _:N0a43dd9ea5e94fe695d8b7df8802cfdd ;
    dct:created "2022-06-15"^^xsd:date ;
    rdfs:isDefinedBy tech: ;
    sw:term_status "accepted"@en ;
    skos:broader tech:Device ;
    skos:definition "Telephone"@en ;
    skos:inScheme tech:tools-classes ;
    skos:prefLabel "Telephone"@en .

tech:iOS a rdfs:Class,
        skos:Concept,
        dpv:Technology ;
    dct:contributor _:N0a43dd9ea5e94fe695d8b7df8802cfdd ;
    dct:created "2022-06-15"^^xsd:date ;
    rdfs:isDefinedBy tech: ;
    sw:term_status "accepted"@en ;
    skos:broader tech:OS ;
    skos:definition "iOS operating system"@en ;
    skos:inScheme tech:tools-classes ;
    skos:prefLabel "iOS"@en .

<https://w3id.org/dpv/tech> a owl:Ontology,
        profile:Profile ;
    dct:bibliographicCitation "Harshvardhan J. Pandit, Beatriz Esteves, Georg P. Krog, Paul Ryan, Delaram Golpayegani, Julian Flake (2025) Data Privacy Vocabulary (DPV) – Version 2.0. In: Demartini, G., et al. The Semantic Web – ISWC 2024. ISWC 2024. Lecture Notes in Computer Science, vol 15233. Springer, Cham. https://doi.org/10.1007/978-3-031-77847-6_10" ;
    dct:conformsTo "http://www.w3.org/2000/01/rdf-schema",
        "http://www.w3.org/2004/02/skos/core" ;
    dct:contributor _:N0a43dd9ea5e94fe695d8b7df8802cfdd,
        _:Ne8d6151e3d8047e6a947b3ec1a3830a1 ;
    dct:created "2024-05-31"@en ;
    dct:creator [ a dct:Agent,
                foaf:Person ;
            org:memberOf [ a foaf:Organization ;
                    foaf:name "Signatu AS" ] ;
            foaf:homepage "https://www.linkedin.com/in/georg-philip-krog-a2a278104/" ;
            foaf:name "Georg P. Krog" ],
        _:N0a43dd9ea5e94fe695d8b7df8802cfdd,
        [ a dct:Agent,
                foaf:Person ;
            scoro:hasORCID "0009-0006-4623-1463" ;
            org:memberOf [ a foaf:Organization ;
                    foaf:name "University of Koblenz" ] ;
            foaf:name "Julian Flake" ],
        [ a dct:Agent,
                foaf:Person ;
            scoro:hasORCID "0000-0003-0770-2737" ;
            org:memberOf [ a foaf:Organization ;
                    foaf:name "Uniphar PLC" ] ;
            foaf:name "Paul Ryan" ],
        _:Ne8d6151e3d8047e6a947b3ec1a3830a1 ;
    dct:description "Extension to the Data Privacy Vocabulary (DPV) providing concepts for representing information about technologies and its provision"@en ;
    dct:identifier "https://w3id.org/dpv/tech" ;
    dct:issued "2024-05-31"@en ;
    dct:license <https://www.w3.org/copyright/document-license-2023/> ;
    dct:modified "2025-03-16"@en ;
    dct:publisher <https://www.w3.org/> ;
    dct:source <https://www.w3.org/groups/cg/dpvcg/> ;
    dct:title "Technology Concepts"@en ;
    bibo:doi "10.5281/zenodo.12505841" ;
    bibo:status "http://purl.org/ontology/bibo/status/published" ;
    vann:preferredNamespacePrefix "tech" ;
    vann:preferredNamespaceUri "https://w3id.org/dpv/tech#" ;
    rdfs:Label "TECH"@en ;
    owl:versionIRI <https://w3id.org/dpv/2.1/tech> ;
    owl:versionInfo "2.1" ;
    profile:hasResource <https://w3id.org/dpv/examples>,
        <https://w3id.org/dpv/guides>,
        <https://w3id.org/dpv/primer>,
        tech:serialisation-html,
        tech:serialisation-jsonld,
        tech:serialisation-n3,
        tech:serialisation-rdf,
        tech:serialisation-ttl ;
    profile:isProfileOf rdfs:,
        skos:,
        <https://w3id.org/dpv> ;
    foaf:logo <https://w3id.org/dpv/media/logo.png> ;
    schema:version "2.1" .

tech:hasAPI a rdf:Property,
        skos:Concept ;
    dcam:domainIncludes dpv:Technology ;
    dcam:rangeIncludes tech:API ;
    dct:contributor _:N0a43dd9ea5e94fe695d8b7df8802cfdd,
        _:Ne8d6151e3d8047e6a947b3ec1a3830a1 ;
    dct:created "2024-12-01"^^xsd:date ;
    rdfs:isDefinedBy tech: ;
    sw:term_status "accepted"@en ;
    skos:definition "Indicates the technology has or uses the associated api"@en ;
    skos:inScheme tech:tools-properties ;
    skos:prefLabel "has api"@en ;
    schema:domainIncludes dpv:Technology ;
    schema:rangeIncludes tech:API .

tech:hasAlgorithm a rdf:Property,
        skos:Concept ;
    dcam:domainIncludes dpv:Technology ;
    dcam:rangeIncludes tech:Algorithm ;
    dct:contributor _:N0a43dd9ea5e94fe695d8b7df8802cfdd,
        _:Ne8d6151e3d8047e6a947b3ec1a3830a1 ;
    dct:created "2024-12-01"^^xsd:date ;
    rdfs:isDefinedBy tech: ;
    sw:term_status "accepted"@en ;
    skos:definition "Indicates the technology has or uses the associated algorithm"@en ;
    skos:inScheme tech:tools-properties ;
    skos:prefLabel "has algorithm"@en ;
    schema:domainIncludes dpv:Technology ;
    schema:rangeIncludes tech:Algorithm .

tech:hasApplication a rdf:Property,
        skos:Concept ;
    dcam:domainIncludes dpv:Technology ;
    dcam:rangeIncludes tech:Application ;
    dct:contributor _:N0a43dd9ea5e94fe695d8b7df8802cfdd,
        _:Ne8d6151e3d8047e6a947b3ec1a3830a1 ;
    dct:created "2024-12-01"^^xsd:date ;
    rdfs:isDefinedBy tech: ;
    sw:term_status "accepted"@en ;
    skos:definition "Indicates the technology has or uses the associated application"@en ;
    skos:inScheme tech:tools-properties ;
    skos:prefLabel "has application"@en ;
    schema:domainIncludes dpv:Technology ;
    schema:rangeIncludes tech:Application .

tech:hasComponent a rdf:Property,
        skos:Concept ;
    dcam:domainIncludes dpv:System ;
    dcam:rangeIncludes tech:Component ;
    dct:contributor _:N0a43dd9ea5e94fe695d8b7df8802cfdd,
        _:Ne8d6151e3d8047e6a947b3ec1a3830a1 ;
    dct:created "2024-12-01"^^xsd:date ;
    rdfs:isDefinedBy tech: ;
    sw:term_status "accepted"@en ;
    skos:definition "Indicates the system has or uses the associated component"@en ;
    skos:inScheme tech:tools-properties ;
    skos:prefLabel "has component"@en ;
    schema:domainIncludes dpv:System ;
    schema:rangeIncludes tech:Component .

tech:hasDevice a rdf:Property,
        skos:Concept ;
    dcam:domainIncludes dpv:Technology ;
    dcam:rangeIncludes tech:Device ;
    dct:contributor _:N0a43dd9ea5e94fe695d8b7df8802cfdd,
        _:Ne8d6151e3d8047e6a947b3ec1a3830a1 ;
    dct:created "2024-12-01"^^xsd:date ;
    rdfs:isDefinedBy tech: ;
    rdfs:subPropertyOf tech:hasHardware ;
    sw:term_status "accepted"@en ;
    skos:broader tech:hasHardware ;
    skos:definition "Indicates the technology has or uses the associated device"@en ;
    skos:inScheme tech:tools-properties ;
    skos:prefLabel "has device"@en ;
    schema:domainIncludes dpv:Technology ;
    schema:rangeIncludes tech:Device .

tech:hasInfrastructure a rdf:Property,
        skos:Concept ;
    dcam:domainIncludes dpv:Technology ;
    dcam:rangeIncludes tech:Infrastructure ;
    dct:contributor _:N0a43dd9ea5e94fe695d8b7df8802cfdd,
        _:Ne8d6151e3d8047e6a947b3ec1a3830a1 ;
    dct:created "2024-12-01"^^xsd:date ;
    rdfs:isDefinedBy tech: ;
    sw:term_status "accepted"@en ;
    skos:definition "Indicates the technology has or uses the associated infrastructure"@en ;
    skos:inScheme tech:tools-properties ;
    skos:prefLabel "has infrastructure"@en ;
    schema:domainIncludes dpv:Technology ;
    schema:rangeIncludes tech:Infrastructure .

tech:hasModel a rdf:Property,
        skos:Concept ;
    dcam:domainIncludes dpv:Technology ;
    dcam:rangeIncludes tech:Model ;
    dct:contributor _:N0a43dd9ea5e94fe695d8b7df8802cfdd,
        _:Ne8d6151e3d8047e6a947b3ec1a3830a1 ;
    dct:created "2024-12-01"^^xsd:date ;
    rdfs:isDefinedBy tech: ;
    sw:term_status "accepted"@en ;
    skos:definition "Indicates the technology has or uses the associated model"@en ;
    skos:inScheme tech:tools-properties ;
    skos:prefLabel "has model"@en ;
    schema:domainIncludes dpv:Technology ;
    schema:rangeIncludes tech:Model .

tech:hasPlatform a rdf:Property,
        skos:Concept ;
    dcam:domainIncludes dpv:Technology ;
    dcam:rangeIncludes tech:Platform ;
    dct:contributor _:N0a43dd9ea5e94fe695d8b7df8802cfdd,
        _:Ne8d6151e3d8047e6a947b3ec1a3830a1 ;
    dct:created "2024-12-01"^^xsd:date ;
    rdfs:isDefinedBy tech: ;
    sw:term_status "accepted"@en ;
    skos:definition "Indicates the technology has or uses the associated platform"@en ;
    skos:inScheme tech:tools-properties ;
    skos:prefLabel "has platform"@en ;
    schema:domainIncludes dpv:Technology ;
    schema:rangeIncludes tech:Platform .

tech:hasService a rdf:Property,
        skos:Concept ;
    dcam:domainIncludes dpv:Technology ;
    dcam:rangeIncludes tech:Service ;
    dct:contributor _:N0a43dd9ea5e94fe695d8b7df8802cfdd,
        _:Ne8d6151e3d8047e6a947b3ec1a3830a1 ;
    dct:created "2024-12-01"^^xsd:date ;
    rdfs:isDefinedBy tech: ;
    sw:term_status "accepted"@en ;
    skos:definition "Indicates the technology has or uses the associated service"@en ;
    skos:inScheme tech:tools-properties ;
    skos:prefLabel "has service"@en ;
    schema:domainIncludes dpv:Technology ;
    schema:rangeIncludes tech:Service .

tech:hasSoftware a rdf:Property,
        skos:Concept ;
    dcam:domainIncludes dpv:Technology ;
    dcam:rangeIncludes tech:Software ;
    dct:contributor _:N0a43dd9ea5e94fe695d8b7df8802cfdd,
        _:Ne8d6151e3d8047e6a947b3ec1a3830a1 ;
    dct:created "2024-12-01"^^xsd:date ;
    rdfs:isDefinedBy tech: ;
    sw:term_status "accepted"@en ;
    skos:definition "Indicates the technology has or uses the associated software"@en ;
    skos:inScheme tech:tools-properties ;
    skos:prefLabel "has software"@en ;
    schema:domainIncludes dpv:Technology ;
    schema:rangeIncludes tech:Software .

tech:hasSystem a rdf:Property,
        skos:Concept ;
    dcam:domainIncludes dpv:Technology ;
    dcam:rangeIncludes tech:System ;
    dct:contributor _:N0a43dd9ea5e94fe695d8b7df8802cfdd,
        _:Ne8d6151e3d8047e6a947b3ec1a3830a1 ;
    dct:created "2024-12-01"^^xsd:date ;
    rdfs:isDefinedBy tech: ;
    sw:term_status "accepted"@en ;
    skos:definition "Indicates the technology has or uses the associated system"@en ;
    skos:inScheme tech:tools-properties ;
    skos:prefLabel "has system"@en ;
    schema:domainIncludes dpv:Technology ;
    schema:rangeIncludes tech:System .

tech:isComponentOf a rdf:Property,
        skos:Concept ;
    dcam:domainIncludes tech:Component ;
    dcam:rangeIncludes dpv:System ;
    dct:contributor _:N0a43dd9ea5e94fe695d8b7df8802cfdd,
        _:Ne8d6151e3d8047e6a947b3ec1a3830a1 ;
    dct:created "2024-12-01"^^xsd:date ;
    rdfs:isDefinedBy tech: ;
    sw:term_status "accepted"@en ;
    skos:definition "Indicates the component is part of the associated system"@en ;
    skos:inScheme tech:tools-properties ;
    skos:prefLabel "is component of"@en ;
    schema:domainIncludes tech:Component ;
    schema:rangeIncludes dpv:System .

tech:serialisation-html a profile:ResourceDescriptor ;
    dct:conformsTo <https://www.w3.org/TR/html/> ;
    dct:format <https://www.iana.org/assignments/media-types/text/html> ;
    dct:title "Technology Concepts - HTML serialiation" ;
    profile:hasArtifact <https://w3id.org/dpv/tech/tech.html> ;
    profile:hasRole role:specification .

tech:serialisation-jsonld a profile:ResourceDescriptor ;
    dct:conformsTo <https://www.w3.org/TR/json-ld11/> ;
    dct:format <https://www.iana.org/assignments/media-types/application/ld+json> ;
    dct:title "Technology Concepts - JSON-LD serialiation" ;
    profile:hasArtifact <https://w3id.org/dpv/tech/tech.jsonld> ;
    profile:hasRole role:vocabulary .

tech:serialisation-n3 a profile:ResourceDescriptor ;
    dct:conformsTo <https://www.w3.org/TeamSubmission/n3/> ;
    dct:format <https://www.iana.org/assignments/media-types/text/n3> ;
    dct:title "Technology Concepts - N3 serialiation" ;
    profile:hasArtifact <https://w3id.org/dpv/tech/tech.n3> ;
    profile:hasRole role:vocabulary .

tech:serialisation-rdf a profile:ResourceDescriptor ;
    dct:conformsTo rdf: ;
    dct:format <https://www.iana.org/assignments/media-types/application/rdf+xml> ;
    dct:title "Technology Concepts - RDF/XML serialiation" ;
    profile:hasArtifact <https://w3id.org/dpv/tech/tech.rdf> ;
    profile:hasRole role:vocabulary .

tech:serialisation-ttl a profile:ResourceDescriptor ;
    dct:conformsTo <https://www.w3.org/TR/turtle/> ;
    dct:format <https://www.iana.org/assignments/media-types/text/turtle> ;
    dct:title "Technology Concepts - Turtle serialiation" ;
    profile:hasArtifact <https://w3id.org/dpv/tech/tech.ttl> ;
    profile:hasRole role:vocabulary .

<https://w3id.org/dpv/examples> a profile:ResourceDescriptor ;
    dct:conformsTo <https://www.w3.org/TR/html/> ;
    dct:format <https://www.iana.org/assignments/media-types/text/html> ;
    dct:title "Examples for Data Privacy Vocabulary" ;
    profile:hasArtifact <https://w3id.org/dpv/examples> ;
    profile:hasRole role:guidance .

<https://w3id.org/dpv/guides> a profile:ResourceDescriptor ;
    dct:conformsTo <https://www.w3.org/TR/html/> ;
    dct:format <https://www.iana.org/assignments/media-types/text/html> ;
    dct:title "Guides for Data Privacy Vocabulary" ;
    profile:hasArtifact <https://w3id.org/dpv/guides> ;
    profile:hasRole role:guidance .

<https://w3id.org/dpv/primer> a profile:ResourceDescriptor ;
    dct:conformsTo <https://www.w3.org/TR/html/> ;
    dct:format <https://www.iana.org/assignments/media-types/text/html> ;
    dct:title "Primer for Data Privacy Vocabulary" ;
    profile:hasArtifact <https://w3id.org/dpv/primer> ;
    profile:hasRole role:guidance .

tech:hasHardware a rdf:Property,
        skos:Concept ;
    dcam:domainIncludes dpv:Technology ;
    dcam:rangeIncludes tech:Hardware ;
    dct:contributor _:N0a43dd9ea5e94fe695d8b7df8802cfdd,
        _:Ne8d6151e3d8047e6a947b3ec1a3830a1 ;
    dct:created "2024-12-01"^^xsd:date ;
    rdfs:isDefinedBy tech: ;
    sw:term_status "accepted"@en ;
    skos:definition "Indicates the technology has or uses the associated hardware"@en ;
    skos:inScheme tech:tools-properties ;
    skos:prefLabel "has hardware"@en ;
    schema:domainIncludes dpv:Technology ;
    schema:rangeIncludes tech:Hardware .

tech:tools-properties a skos:ConceptScheme .

tech:tools-classes a skos:ConceptScheme .

_:N2107ae3007164122b8f508ef58f07bab a foaf:Organization ;
    foaf:name "ADAPT Centre, Trinity College Dublin" .

_:N313d89a6c37147bfac1bbb4aa7f6510b a foaf:Organization ;
    foaf:name "ADAPT Centre, Dublin City University" .

_:Ne8d6151e3d8047e6a947b3ec1a3830a1 a dct:Agent,
        foaf:Person ;
    scoro:hasORCID "0000-0002-1208-186X" ;
    org:memberOf _:N2107ae3007164122b8f508ef58f07bab ;
    foaf:name "Delaram Golpayegani" .

_:N0a43dd9ea5e94fe695d8b7df8802cfdd a dct:Agent,
        foaf:Person ;
    scoro:hasORCID "0000-0002-5068-3714" ;
    org:memberOf _:N313d89a6c37147bfac1bbb4aa7f6510b ;
    foaf:homepage "https://harshp.com/" ;
    foaf:name "Harshvardhan J. Pandit" .

