@prefix dct: <http://purl.org/dc/terms/> .
@prefix dpv: <http://www.w3.org/ns/dpv#> .
@prefix ns1: <http://purl.org/vocab/vann/> .
@prefix odrl: <http://www.w3.org/ns/odrl/2/> .
@prefix owl: <http://www.w3.org/2002/07/owl#> .
@prefix prov: <http://www.w3.org/ns/prov#> .
@prefix rdf: <http://www.w3.org/1999/02/22-rdf-syntax-ns#> .
@prefix rdfs: <http://www.w3.org/2000/01/rdf-schema#> .
@prefix spl: <http://www.specialprivacy.eu/langs/usage-policy#> .
@prefix svd: <http://www.specialprivacy.eu/vocabs/data#> .
@prefix svpr: <http://www.specialprivacy.eu/vocabs/processing#> .
@prefix svpu: <http://www.specialprivacy.eu/vocabs/purposes#> .
@prefix sw: <http://www.w3.org/2003/06/sw-vocab-status/ns#> .
@prefix time: <http://www.w3.org/2006/time#> .
@prefix xsd: <http://www.w3.org/2001/XMLSchema#> .

dpv:AcademicResearch a rdfs:Class ;
    rdfs:label "Academic Research"@en ;
    dct:created "2018-12-10"^^xsd:date ;
    dct:creator "Axel Polleres"^^xsd:string,
        "Elmar Kiesling"^^xsd:string,
        "Fajar Ekaputra"^^xsd:string,
        "Harshvardhan J. Pandit"^^xsd:string,
        "Javier Fernandez"^^xsd:string,
        "Simon Steyskal"^^xsd:string ;
    dct:date-accepted "2019-04-05"^^xsd:date ;
    dct:description "Research conducted in an academic context e.g. within universities"@en ;
    rdfs:isDefinedBy <https://www.w3.org/community/dpvcg/wiki/Purposes_for_handling_Personal_Data#High-level_categories_.28to-be-discussed.29> ;
    rdfs:seeAlso svpu:Education ;
    rdfs:subClassOf dpv:ResearchAndDevelopment ;
    sw:term_status "accepted"@en .

dpv:Accent a rdfs:Class ;
    rdfs:label "Accent"@en ;
    dct:created "2019-04-04"^^xsd:date ;
    dct:creator "Elmar Kiesling; Harshvardhan J. Pandit"^^xsd:string,
        "Fajar Ekaputra"^^xsd:string ;
    dct:date-accepted "2019-06-04"^^xsd:date ;
    dct:description "Information about an individual’s accent."@en ;
    rdfs:isDefinedBy <https://enterprivacy.com/wp-content/uploads/2018/09/Categories-of-Personal-Information.pdf> ;
    rdfs:subClassOf dpv:Language ;
    sw:term_status "accepted"@en .

dpv:AccessControl a rdfs:Class ;
    rdfs:label "Access Control"@en ;
    dct:created "2018-12-10"^^xsd:date ;
    dct:creator "Axel Polleres"^^xsd:string,
        "Elmar Kiesling"^^xsd:string,
        "Fajar Ekaputra"^^xsd:string,
        "Harshvardhan J. Pandit"^^xsd:string,
        "Javier Fernandez"^^xsd:string,
        "Simon Steyskal"^^xsd:string ;
    dct:date-accepted "2019-04-05"^^xsd:date ;
    dct:description "To conduct or enforce access control"@en ;
    rdfs:isDefinedBy <https://www.w3.org/community/dpvcg/wiki/Purposes_for_handling_Personal_Data#High-level_categories_.28to-be-discussed.29> ;
    rdfs:seeAlso svpu:Login ;
    rdfs:subClassOf dpv:Security ;
    sw:term_status "accepted"@en .

dpv:AccessControlMethod a rdfs:Class ;
    rdfs:label "Access Control Method"@en ;
    dct:created "2019-04-04"^^xsd:date ;
    dct:creator "Axel Polleres"^^xsd:string,
        "Harshvardhan J. Pandit"^^xsd:string,
        "Mark Lizar"^^xsd:string,
        "Rob Brennan"^^xsd:string ;
    dct:date-accepted "2019-04-05"^^xsd:date ;
    dct:description "methods which restrict access to a place or resource"@en ;
    rdfs:isDefinedBy "DPVCG"^^xsd:string ;
    rdfs:subClassOf dpv:TechnicalMeasure ;
    sw:term_status "accepted"@en .

dpv:AccountIdentifier a rdfs:Class ;
    rdfs:label "Account Identifier"@en ;
    dct:created "2019-04-04"^^xsd:date ;
    dct:creator "Elmar Kiesling; Harshvardhan J. Pandit"^^xsd:string,
        "Fajar Ekaputra"^^xsd:string ;
    dct:date-accepted "2019-06-04"^^xsd:date ;
    dct:description "Information about an individual's financial account identifier."@en ;
    rdfs:isDefinedBy <https://enterprivacy.com/wp-content/uploads/2018/09/Categories-of-Personal-Information.pdf> ;
    rdfs:subClassOf dpv:FinancialAccount ;
    sw:term_status "accepted"@en .

dpv:Acquantaince a rdfs:Class ;
    rdfs:label "Acquantaince"@en ;
    dct:created "2019-04-04"^^xsd:date ;
    dct:creator "Elmar Kiesling; Harshvardhan J. Pandit"^^xsd:string,
        "Fajar Ekaputra"^^xsd:string ;
    dct:date-accepted "2019-06-04"^^xsd:date ;
    dct:description "Information about acquaintainces in a social network."@en ;
    rdfs:isDefinedBy <https://enterprivacy.com/wp-content/uploads/2018/09/Categories-of-Personal-Information.pdf> ;
    rdfs:subClassOf dpv:SocialNetwork ;
    sw:term_status "accepted"@en .

dpv:Acquire a rdfs:Class ;
    rdfs:label "Acquire"@en ;
    dct:created "2019-04-04"^^xsd:date ;
    dct:date-accepted "2019-05-07"^^xsd:date ;
    dct:description "to come into possession or control of the data"@en ;
    rdfs:isDefinedBy "DPVCG"^^xsd:string ;
    rdfs:subClassOf dpv:Obtain ;
    sw:term_status "accepted"@en .

dpv:Adapt a rdfs:Class ;
    rdfs:label "Adapt"@en ;
    dct:created "2019-04-04"^^xsd:date ;
    dct:date-accepted "2019-05-07"^^xsd:date ;
    dct:description "to modify the data, often rewritten into a new form for a new use"@en ;
    rdfs:isDefinedBy <https://eur-lex.europa.eu/eli/reg/2016/679/art_4/par_2/oj> ;
    rdfs:subClassOf dpv:Transform ;
    sw:term_status "accepted"@en .

dpv:Advertising a rdfs:Class ;
    rdfs:label "Advertising"@en ;
    dct:created "2020-07-08"^^xsd:date ;
    dct:creator "Beatriz"^^xsd:string,
        "Georg"^^xsd:string,
        "Harsh"^^xsd:string ;
    dct:description "Process or Artefact which is used to call attention to a product, service, etc. through announcements, notices, or other forms of communication."@en ;
    rdfs:comment "Advertising by itself is a subset of Marketing. Advertising by itself does not indicate 'personalisation' i.e. personalised ads."@en ;
    sw:term_status "proposed"@en .

dpv:Age a rdfs:Class ;
    rdfs:label "Age"@en ;
    dct:created "2019-04-04"^^xsd:date ;
    dct:creator "Elmar Kiesling; Harshvardhan J. Pandit"^^xsd:string,
        "Fajar Ekaputra"^^xsd:string ;
    dct:date-accepted "2019-06-04"^^xsd:date ;
    dct:description "Information about an individual's age"@en ;
    rdfs:isDefinedBy <https://enterprivacy.com/wp-content/uploads/2018/09/Categories-of-Personal-Information.pdf> ;
    rdfs:subClassOf dpv:PhysicalCharacteristic ;
    sw:term_status "accepted"@en .

dpv:Align a rdfs:Class ;
    rdfs:label "Align"@en ;
    dct:created "2019-04-04"^^xsd:date ;
    dct:date-accepted "2019-05-07"^^xsd:date ;
    dct:description "to adjust the data to be in relation to another data"@en ;
    rdfs:isDefinedBy <https://eur-lex.europa.eu/eli/reg/2016/679/art_4/par_2/oj> ;
    rdfs:subClassOf dpv:Transform ;
    sw:term_status "accepted"@en .

dpv:Alter a rdfs:Class ;
    rdfs:label "Alter"@en ;
    dct:created "2019-04-04"^^xsd:date ;
    dct:date-accepted "2019-05-07"^^xsd:date ;
    dct:description "to change the data withouth changing it into something else"@en ;
    rdfs:isDefinedBy <https://eur-lex.europa.eu/eli/reg/2016/679/art_4/par_2/oj> ;
    rdfs:subClassOf dpv:Transform ;
    sw:term_status "accepted"@en .

dpv:Analyse a rdfs:Class ;
    rdfs:label "Analyse"@en ;
    dct:created "2019-04-04"^^xsd:date ;
    dct:date-accepted "2019-05-07"^^xsd:date ;
    dct:description "to study or examine the data in detail"@en ;
    rdfs:isDefinedBy <https://www.specialprivacy.eu/vocabs/processing> ;
    rdfs:seeAlso svpr:Analyse ;
    rdfs:subClassOf dpv:Use ;
    sw:term_status "accepted"@en .

dpv:Anonymise a rdfs:Class ;
    rdfs:label "Anonymise"@en ;
    dct:created "2019-04-04"^^xsd:date ;
    dct:date-accepted "2019-05-07"^^xsd:date ;
    dct:description "to irreversibly alter personal data in such a way that a unique data subject can no longer be identified directly or indirectly or in combination with other data"@en ;
    rdfs:isDefinedBy <https://www.specialprivacy.eu/vocabs/processing> ;
    rdfs:seeAlso svpr:Anonymize ;
    rdfs:subClassOf dpv:Transform ;
    sw:term_status "accepted"@en .

dpv:Anonymization a rdfs:Class ;
    rdfs:label "Anonymization"@en ;
    dct:created "2019-04-04"^^xsd:date ;
    dct:creator "Axel Polleres"^^xsd:string,
        "Harshvardhan J. Pandit"^^xsd:string,
        "Mark Lizar"^^xsd:string,
        "Rob Brennan"^^xsd:string ;
    dct:date-accepted "2019-04-05"^^xsd:date ;
    dct:description "process by which personal data is irreversibly altered in such a way that a data subject can no longer be identified directly or indirectly, either by the data controller alone or in collaboration with any other party"@en ;
    rdfs:isDefinedBy "ISO 25237"^^xsd:string ;
    rdfs:subClassOf dpv:PseudoAnonymization ;
    sw:term_status "accepted"@en .

dpv:ApartmentOwned a rdfs:Class ;
    rdfs:label "Apartment Owned"@en ;
    dct:created "2019-04-04"^^xsd:date ;
    dct:creator "Elmar Kiesling; Harshvardhan J. Pandit"^^xsd:string,
        "Fajar Ekaputra"^^xsd:string ;
    dct:date-accepted "2019-06-04"^^xsd:date ;
    dct:description "Information on the apartement(s) owned by an individual."@en ;
    rdfs:isDefinedBy <https://enterprivacy.com/wp-content/uploads/2018/09/Categories-of-Personal-Information.pdf> ;
    rdfs:subClassOf dpv:HouseOwned ;
    sw:term_status "accepted"@en .

dpv:Association a rdfs:Class ;
    rdfs:label "Association"@en ;
    dct:created "2019-04-04"^^xsd:date ;
    dct:creator "Elmar Kiesling; Harshvardhan J. Pandit"^^xsd:string,
        "Fajar Ekaputra"^^xsd:string ;
    dct:date-accepted "2019-06-04"^^xsd:date ;
    dct:description "Information about associations in a social network with other individuals, groups, or entities e.g. friend of a friend"@en ;
    rdfs:isDefinedBy <https://enterprivacy.com/wp-content/uploads/2018/09/Categories-of-Personal-Information.pdf> ;
    rdfs:subClassOf dpv:SocialNetwork ;
    sw:term_status "accepted"@en .

dpv:Attitude a rdfs:Class ;
    rdfs:label "Attitude"@en ;
    dct:created "2019-04-04"^^xsd:date ;
    dct:creator "Elmar Kiesling; Harshvardhan J. Pandit"^^xsd:string,
        "Fajar Ekaputra"^^xsd:string ;
    dct:date-accepted "2019-06-04"^^xsd:date ;
    dct:description "Information that relates to an individual's attitude."@en ;
    rdfs:isDefinedBy <https://enterprivacy.com/wp-content/uploads/2018/09/Categories-of-Personal-Information.pdf> ;
    rdfs:subClassOf dpv:Behavioral ;
    sw:term_status "accepted"@en .

dpv:Authenticating a rdfs:Class ;
    rdfs:label "Authenticating"@en ;
    dct:created "2019-04-04"^^xsd:date ;
    dct:creator "Elmar Kiesling; Harshvardhan J. Pandit"^^xsd:string,
        "Fajar Ekaputra"^^xsd:string ;
    dct:date-accepted "2019-06-04"^^xsd:date ;
    dct:description "Information used to authenticate an individual with something they know"@en ;
    rdfs:isDefinedBy <https://enterprivacy.com/wp-content/uploads/2018/09/Categories-of-Personal-Information.pdf> ;
    rdfs:subClassOf dpv:Internal ;
    sw:term_status "accepted"@en .

dpv:AuthenticationProtocols a rdfs:Class ;
    rdfs:label "Authentication Protocols"@en ;
    dct:created "2019-04-04"^^xsd:date ;
    dct:creator "Axel Polleres"^^xsd:string,
        "Harshvardhan J. Pandit"^^xsd:string,
        "Mark Lizar"^^xsd:string,
        "Rob Brennan"^^xsd:string ;
    dct:date-accepted "2019-04-05"^^xsd:date ;
    dct:description "protocols involving validation of identity i.e. authentication of a person or information"@en ;
    rdfs:isDefinedBy "DPVCG"^^xsd:string ;
    rdfs:subClassOf dpv:TechnicalMeasure ;
    sw:term_status "accepted"@en .

dpv:AuthorisationProcedure a rdfs:Class ;
    rdfs:label "Authorisation Procedure"@en ;
    dct:created "2019-04-04"^^xsd:date ;
    dct:creator "Axel Polleres"^^xsd:string,
        "Harshvardhan J. Pandit"^^xsd:string,
        "Mark Lizar"^^xsd:string,
        "Rob Brennan"^^xsd:string ;
    dct:date-accepted "2019-04-05"^^xsd:date ;
    dct:description "Specifies procedures for determining permission or authority"@en ;
    rdfs:comment "non-technical authorisation procedures: How is it described on an organisational level, who gets access to the data"@en ;
    rdfs:isDefinedBy "DPVCG"^^xsd:string ;
    rdfs:subClassOf dpv:OrganisationalMeasure ;
    sw:term_status "accepted"@en .

dpv:BankAccount a rdfs:Class ;
    rdfs:label "Bank Account"@en ;
    dct:created "2019-04-04"^^xsd:date ;
    dct:creator "Elmar Kiesling; Harshvardhan J. Pandit"^^xsd:string,
        "Fajar Ekaputra"^^xsd:string ;
    dct:date-accepted "2019-06-04"^^xsd:date ;
    dct:description "Information related to an individual's bank account."@en ;
    rdfs:isDefinedBy <https://enterprivacy.com/wp-content/uploads/2018/09/Categories-of-Personal-Information.pdf> ;
    rdfs:subClassOf dpv:FinancialAccount ;
    sw:term_status "accepted"@en .

dpv:Behavioral a rdfs:Class ;
    rdfs:label "Behavioral"@en ;
    dct:created "2019-04-04"^^xsd:date ;
    dct:creator "Elmar Kiesling; Harshvardhan J. Pandit"^^xsd:string,
        "Fajar Ekaputra"^^xsd:string ;
    dct:date-accepted "2019-06-04"^^xsd:date ;
    dct:description "Information that describes an individual’s behavior or activity, on-line or off"@en ;
    rdfs:isDefinedBy <https://enterprivacy.com/wp-content/uploads/2018/09/Categories-of-Personal-Information.pdf> ;
    rdfs:seeAlso svd:Activity ;
    rdfs:subClassOf dpv:External ;
    sw:term_status "accepted"@en .

dpv:Beneficiary a rdfs:Class ;
    rdfs:label "Beneficiary"@en ;
    dct:created "2019-05-23"^^xsd:date ;
    dct:description "self.DataSubject, self.DataController, society ? ( --- under consideration ---)"@en ;
    rdfs:comment "This needs further details, the group is asking feedback about whether Beneficiaries of a specific purposes hould be specified separately or not"@en ;
    sw:term_status "proposed"@en .

dpv:Biometric a rdfs:Class ;
    rdfs:label "Biometric"@en ;
    dct:created "2019-04-04"^^xsd:date ;
    dct:creator "Elmar Kiesling; Harshvardhan J. Pandit"^^xsd:string,
        "Fajar Ekaputra"^^xsd:string ;
    dct:date-accepted "2019-06-04"^^xsd:date ;
    dct:description "Biometric information on an individual."@en ;
    rdfs:isDefinedBy <https://enterprivacy.com/wp-content/uploads/2018/09/Categories-of-Personal-Information.pdf> ;
    rdfs:subClassOf dpv:Identifying,
        dpv:SpecialCategoryPersonalData ;
    sw:term_status "accepted"@en .

dpv:BloodType a rdfs:Class ;
    rdfs:label "Blood Type"@en ;
    dct:created "2019-04-04"^^xsd:date ;
    dct:creator "Elmar Kiesling; Harshvardhan J. Pandit"^^xsd:string,
        "Fajar Ekaputra"^^xsd:string ;
    dct:date-accepted "2019-06-04"^^xsd:date ;
    dct:description "Information about an individual's blood type."@en ;
    rdfs:isDefinedBy <https://enterprivacy.com/wp-content/uploads/2018/09/Categories-of-Personal-Information.pdf> ;
    rdfs:subClassOf dpv:MedicalHealth ;
    sw:term_status "accepted"@en .

dpv:BrowserFingerprint a rdfs:Class ;
    rdfs:label "Browser Fingerprint"@en ;
    dct:created "2019-04-04"^^xsd:date ;
    dct:creator "Elmar Kiesling; Harshvardhan J. Pandit"^^xsd:string,
        "Fajar Ekaputra"^^xsd:string ;
    dct:date-accepted "2019-06-04"^^xsd:date ;
    dct:description "Information that characterizes the browser used by an individual, which in turn can be used to uniquely identify a user."@en ;
    rdfs:isDefinedBy <https://enterprivacy.com/wp-content/uploads/2018/09/Categories-of-Personal-Information.pdf> ;
    rdfs:subClassOf dpv:DeviceBased ;
    sw:term_status "accepted"@en .

dpv:BrowsingBehavior a rdfs:Class ;
    rdfs:label "Browsing Behavior"@en ;
    dct:created "2019-04-04"^^xsd:date ;
    dct:creator "Elmar Kiesling; Harshvardhan J. Pandit"^^xsd:string,
        "Fajar Ekaputra"^^xsd:string ;
    dct:date-accepted "2019-06-04"^^xsd:date ;
    dct:description "Information that relates to an individual's browsing behaviour."@en ;
    rdfs:isDefinedBy <https://enterprivacy.com/wp-content/uploads/2018/09/Categories-of-Personal-Information.pdf> ;
    rdfs:seeAlso svd:OnlineActivity ;
    rdfs:subClassOf dpv:Behavioral ;
    sw:term_status "accepted"@en .

dpv:CallLog a rdfs:Class ;
    rdfs:label "Call Log"@en ;
    dct:created "2019-04-04"^^xsd:date ;
    dct:creator "Elmar Kiesling; Harshvardhan J. Pandit"^^xsd:string,
        "Fajar Ekaputra"^^xsd:string ;
    dct:date-accepted "2019-06-04"^^xsd:date ;
    dct:description "Information on the calls that an individual has made."@en ;
    rdfs:isDefinedBy <https://enterprivacy.com/wp-content/uploads/2018/09/Categories-of-Personal-Information.pdf> ;
    rdfs:subClassOf dpv:Behavioral ;
    sw:term_status "accepted"@en .

dpv:CarOwned a rdfs:Class ;
    rdfs:label "Car Owned"@en ;
    dct:created "2019-04-04"^^xsd:date ;
    dct:creator "Elmar Kiesling; Harshvardhan J. Pandit"^^xsd:string,
        "Fajar Ekaputra"^^xsd:string ;
    dct:date-accepted "2019-06-04"^^xsd:date ;
    dct:description "Information about cars owned by an individual."@en ;
    rdfs:isDefinedBy <https://enterprivacy.com/wp-content/uploads/2018/09/Categories-of-Personal-Information.pdf> ;
    rdfs:subClassOf dpv:Ownership ;
    sw:term_status "accepted"@en .

dpv:Certification a rdfs:Class ;
    rdfs:label "Certification"@en,
        "ProfessionalCertification"@en ;
    dct:created "2019-04-04"^^xsd:date ;
    dct:creator "Axel Polleres"^^xsd:string,
        "Elmar Kiesling; Harshvardhan J. Pandit"^^xsd:string,
        "Fajar Ekaputra"^^xsd:string,
        "Harshvardhan J. Pandit"^^xsd:string,
        "Mark Lizar"^^xsd:string,
        "Rob Brennan"^^xsd:string ;
    dct:date-accepted "2019-04-05"^^xsd:date,
        "2019-06-04"^^xsd:date ;
    dct:description "Information about professional certifications associated with an individual"@en,
        "certification mechanisms, seals, and marks for the purpose of demonstrating compliance"@en ;
    rdfs:isDefinedBy <https://enterprivacy.com/wp-content/uploads/2018/09/Categories-of-Personal-Information.pdf>,
        "DPVCG"^^xsd:string ;
    rdfs:subClassOf dpv:CertificationSeal,
        dpv:Professional ;
    sw:term_status "accepted"@en .

dpv:CertificationSeal a rdfs:Class ;
    rdfs:label "Certification and Seal"@en ;
    dct:created "2019-04-04"^^xsd:date ;
    dct:creator "Axel Polleres"^^xsd:string,
        "Harshvardhan J. Pandit"^^xsd:string,
        "Mark Lizar"^^xsd:string,
        "Rob Brennan"^^xsd:string ;
    dct:date-accepted "2019-04-05"^^xsd:date ;
    dct:description "Category of certifications, seals, and marks indicating compliance to regulations or practices"@en ;
    rdfs:isDefinedBy "DPVCG"^^xsd:string ;
    rdfs:subClassOf dpv:OrganisationalMeasure ;
    sw:term_status "accepted"@en .

dpv:Character a rdfs:Class ;
    rdfs:label "Character"@en ;
    dct:created "2019-04-04"^^xsd:date ;
    dct:creator "Elmar Kiesling; Harshvardhan J. Pandit"^^xsd:string,
        "Fajar Ekaputra"^^xsd:string ;
    dct:date-accepted "2019-06-04"^^xsd:date ;
    dct:description "Information about an individual's character in the public sphere"@en ;
    rdfs:isDefinedBy <https://enterprivacy.com/wp-content/uploads/2018/09/Categories-of-Personal-Information.pdf> ;
    rdfs:subClassOf dpv:PublicLife ;
    sw:term_status "accepted"@en .

dpv:Child a rdfs:Class ;
    rdfs:label "Child"@en ;
    dct:created "2019-06-06"^^xsd:date ;
    dct:creator "Harshvardhan J. Pandit"^^xsd:string ;
    dct:description "A 'child' is a natural legal person who is below a certain legal age depending on the legal jurisdiction."@en ;
    rdfs:comment "A 'child' is distinct from a 'minor'. For example, the legal age for a 'minor' in most countries is 18, whereas a 'child' can be a minor below the age of 14."@en ;
    rdfs:subClassOf dpv:DataSubject ;
    sw:term_status "proposed"@en .

dpv:CodeOfConduct a rdfs:Class ;
    rdfs:label "Code of Conduct"@en ;
    dct:created "2019-04-04"^^xsd:date ;
    dct:creator "Axel Polleres"^^xsd:string,
        "Harshvardhan J. Pandit"^^xsd:string,
        "Mark Lizar"^^xsd:string,
        "Rob Brennan"^^xsd:string ;
    dct:date-accepted "2019-04-05"^^xsd:date ;
    dct:description "A set of rules or procedures outlining the norms and practices for conducting activities"@en ;
    rdfs:isDefinedBy "DPVCG"^^xsd:string ;
    rdfs:subClassOf dpv:GuidelinesPrinciple ;
    sw:term_status "accepted"@en .

dpv:Collect a rdfs:Class ;
    rdfs:label "Collect"@en ;
    dct:created "2019-04-04"^^xsd:date ;
    dct:date-accepted "2019-05-07"^^xsd:date ;
    dct:description "to gather data from someone"@en ;
    rdfs:isDefinedBy <https://eur-lex.europa.eu/eli/reg/2016/679/art_4/par_2/oj>,
        <https://www.specialprivacy.eu/vocabs/processing> ;
    rdfs:seeAlso svpr:Collect ;
    rdfs:subClassOf dpv:Obtain ;
    sw:term_status "accepted"@en .

dpv:Combine a rdfs:Class ;
    rdfs:label "Combine"@en ;
    dct:created "2019-04-04"^^xsd:date ;
    dct:date-accepted "2019-05-07"^^xsd:date ;
    dct:description "to join or merge data"@en ;
    rdfs:isDefinedBy <https://eur-lex.europa.eu/eli/reg/2016/679/art_4/par_2/oj>,
        <https://www.specialprivacy.eu/vocabs/processing> ;
    rdfs:seeAlso svpr:Aggregate ;
    rdfs:subClassOf dpv:Transform ;
    sw:term_status "accepted"@en .

dpv:CommercialInterest a rdfs:Class ;
    rdfs:label "Commercial Interest"@en ;
    dct:created "2018-12-10"^^xsd:date ;
    dct:creator "Axel Polleres"^^xsd:string,
        "Elmar Kiesling"^^xsd:string,
        "Fajar Ekaputra"^^xsd:string,
        "Harshvardhan J. Pandit"^^xsd:string,
        "Javier Fernandez"^^xsd:string,
        "Simon Steyskal"^^xsd:string ;
    dct:date-accepted "2019-04-05"^^xsd:date ;
    dct:description "For purposes of commercial activities i.e. of profit or benefit to the Controller"@en ;
    rdfs:isDefinedBy <https://www.w3.org/community/dpvcg/wiki/Purposes_for_handling_Personal_Data#High-level_categories_.28to-be-discussed.29> ;
    rdfs:subClassOf dpv:Purpose ;
    sw:term_status "accepted"@en .

dpv:CommercialResearch a rdfs:Class ;
    rdfs:label "Commercial Research"@en ;
    dct:created "2018-12-10"^^xsd:date ;
    dct:creator "Axel Polleres"^^xsd:string,
        "Elmar Kiesling"^^xsd:string,
        "Fajar Ekaputra"^^xsd:string,
        "Harshvardhan J. Pandit"^^xsd:string,
        "Javier Fernandez"^^xsd:string,
        "Simon Steyskal"^^xsd:string ;
    dct:date-accepted "2019-04-05"^^xsd:date ;
    dct:description "Research conducted in a commercial setting e.g. in a company"@en ;
    rdfs:isDefinedBy <https://www.w3.org/community/dpvcg/wiki/Purposes_for_handling_Personal_Data#High-level_categories_.28to-be-discussed.29> ;
    rdfs:seeAlso svpu:Develop ;
    rdfs:subClassOf dpv:ResearchAndDevelopment ;
    sw:term_status "accepted"@en .

dpv:Communication a rdfs:Class ;
    rdfs:label "Communication"@en ;
    dct:created "2019-04-04"^^xsd:date ;
    dct:creator "Elmar Kiesling; Harshvardhan J. Pandit"^^xsd:string,
        "Fajar Ekaputra"^^xsd:string ;
    dct:date-accepted "2019-06-04"^^xsd:date ;
    dct:description "Information communicated from or to an individual"@en ;
    rdfs:isDefinedBy <https://enterprivacy.com/wp-content/uploads/2018/09/Categories-of-Personal-Information.pdf> ;
    rdfs:subClassOf dpv:Social ;
    sw:term_status "accepted"@en .

dpv:CommunicationsMetadata a rdfs:Class ;
    rdfs:label "Communications Metadata"@en ;
    dct:created "2019-04-04"^^xsd:date ;
    dct:creator "Elmar Kiesling; Harshvardhan J. Pandit"^^xsd:string,
        "Fajar Ekaputra"^^xsd:string ;
    dct:date-accepted "2019-06-04"^^xsd:date ;
    dct:description "Information about communication metadata in the public sphere"@en ;
    rdfs:isDefinedBy <https://enterprivacy.com/wp-content/uploads/2018/09/Categories-of-Personal-Information.pdf> ;
    rdfs:seeAlso svd:Interactive ;
    rdfs:subClassOf dpv:PublicLife ;
    sw:term_status "accepted"@en .

dpv:Connection a rdfs:Class ;
    rdfs:label "Connection"@en ;
    dct:created "2019-04-04"^^xsd:date ;
    dct:creator "Elmar Kiesling; Harshvardhan J. Pandit"^^xsd:string,
        "Fajar Ekaputra"^^xsd:string ;
    dct:date-accepted "2019-06-04"^^xsd:date ;
    dct:description "Information about and including connections of an individual in a social network"@en ;
    rdfs:isDefinedBy <https://enterprivacy.com/wp-content/uploads/2018/09/Categories-of-Personal-Information.pdf> ;
    rdfs:subClassOf dpv:SocialNetwork ;
    sw:term_status "accepted"@en .

dpv:Consent a rdfs:Class ;
    rdfs:label "Consent"@en ;
    dct:created "2019-04-04"^^xsd:date ;
    dct:date-accepted "2019-04-05"^^xsd:date ;
    dct:description "Consent as defined by Article 4(11) of the GDPR"@en ;
    rdfs:isDefinedBy <https://eur-lex.europa.eu/eli/reg/2016/679/art_4/par_11/oj> ;
    sw:term_status "accepted"@en .

dpv:Consult a rdfs:Class ;
    rdfs:label "Consult"@en ;
    dct:created "2019-04-04"^^xsd:date ;
    dct:date-accepted "2019-05-07"^^xsd:date ;
    dct:description "to consult or query data"@en ;
    rdfs:isDefinedBy <https://eur-lex.europa.eu/eli/reg/2016/679/art_4/par_2/oj>,
        <https://www.specialprivacy.eu/vocabs/processing> ;
    rdfs:seeAlso svpr:Query ;
    rdfs:subClassOf dpv:Use ;
    sw:term_status "accepted"@en .

dpv:Contact a rdfs:Class ;
    rdfs:label "Contact"@en ;
    dct:created "2019-04-04"^^xsd:date ;
    dct:creator "Elmar Kiesling; Harshvardhan J. Pandit"^^xsd:string,
        "Fajar Ekaputra"^^xsd:string ;
    dct:date-accepted "2019-06-04"^^xsd:date ;
    dct:description "Information that can be used for contacting an individual e.g. email address or phone number"@en ;
    rdfs:isDefinedBy <https://enterprivacy.com/wp-content/uploads/2018/09/Categories-of-Personal-Information.pdf> ;
    rdfs:seeAlso svd:Physical ;
    rdfs:subClassOf dpv:Tracking ;
    sw:term_status "accepted"@en .

dpv:Context a rdfs:Class ;
    rdfs:label "Context"@en ;
    dct:created "2019-04-04"^^xsd:date ;
    dct:date-accepted "2019-04-05"^^xsd:date ;
    dct:description "Used to scope the purpose, e.g. restriction to a certain business sector"@en ;
    sw:term_status "accepted"@en .

dpv:Contract a rdfs:Class ;
    rdfs:label "Contract"@en ;
    dct:created "2019-04-04"^^xsd:date ;
    dct:creator "Axel Polleres"^^xsd:string,
        "Harshvardhan J. Pandit"^^xsd:string,
        "Mark Lizar"^^xsd:string,
        "Rob Brennan"^^xsd:string ;
    dct:date-accepted "2019-04-05"^^xsd:date ;
    dct:description "Contractual terms governing data handling within the data controller"@en ;
    rdfs:isDefinedBy "DPVCG"^^xsd:string ;
    rdfs:subClassOf dpv:LegalAgreement ;
    sw:term_status "accepted"@en .

dpv:Copy a rdfs:Class ;
    rdfs:label "Copy"@en ;
    dct:created "2019-04-04"^^xsd:date ;
    dct:date-accepted "2019-05-07"^^xsd:date ;
    dct:description "to produce an exact reprodution of the data"@en ;
    rdfs:isDefinedBy <https://www.specialprivacy.eu/vocabs/processing> ;
    rdfs:seeAlso svpr:Copy ;
    rdfs:subClassOf dpv:Processing ;
    sw:term_status "accepted"@en .

dpv:Country a rdfs:Class ;
    rdfs:label "Country"@en ;
    dct:created "2019-04-04"^^xsd:date ;
    dct:creator "Elmar Kiesling; Harshvardhan J. Pandit"^^xsd:string,
        "Fajar Ekaputra"^^xsd:string ;
    dct:date-accepted "2019-06-04"^^xsd:date ;
    dct:description "Information about an individual’s country e.g. residence, travel."@en ;
    rdfs:comment "ISSUE-24"@en ;
    rdfs:isDefinedBy <https://enterprivacy.com/wp-content/uploads/2018/09/Categories-of-Personal-Information.pdf> ;
    rdfs:subClassOf dpv:Location ;
    sw:term_status "accepted"@en .

dpv:CreateEventRecommendations a rdfs:Class ;
    rdfs:label "Create Event Recommendations"@en ;
    dct:created "2019-11-25"^^xsd:date ;
    dct:creator "Harshvardhan J. Pandit"^^xsd:string,
        "Rudy Jacob"^^xsd:string ;
    dct:date-accepted "2019-11-26"^^xsd:date ;
    dct:description "Create and provide personalised recommendations for events to the individual"@en ;
    rdfs:isDefinedBy "SPECIAL"^^xsd:string ;
    rdfs:subClassOf dpv:CreatePersonalizedRecommendations ;
    sw:term_status "accepted"@en .

dpv:CreatePersonalizedRecommendations a rdfs:Class ;
    rdfs:label "Create Personalized Recommendations"@en ;
    dct:created "2019-11-25"^^xsd:date ;
    dct:creator "Harshvardhan J. Pandit"^^xsd:string,
        "Rudy Jacob"^^xsd:string ;
    dct:date-accepted "2019-11-26"^^xsd:date ;
    dct:description "Create and provide personalised recommendations to the individual"@en ;
    rdfs:isDefinedBy "SPECIAL"^^xsd:string ;
    rdfs:subClassOf dpv:ServicePersonalization ;
    sw:term_status "accepted"@en .

dpv:CreateProductRecommendations a rdfs:Class ;
    rdfs:label "Create Product Recommendations"@en ;
    dct:created "2018-12-10"^^xsd:date ;
    dct:creator "Axel Polleres"^^xsd:string,
        "Elmar Kiesling"^^xsd:string,
        "Fajar Ekaputra"^^xsd:string,
        "Harshvardhan J. Pandit"^^xsd:string,
        "Javier Fernandez"^^xsd:string,
        "Simon Steyskal"^^xsd:string ;
    dct:date-accepted "2019-04-05"^^xsd:date ;
    dct:description "To create product recommendations e.g. suggest similar products"@en ;
    rdfs:isDefinedBy <https://www.w3.org/community/dpvcg/wiki/Purposes_for_handling_Personal_Data#High-level_categories_.28to-be-discussed.29> ;
    rdfs:seeAlso svpu:Marketing ;
    rdfs:subClassOf dpv:CreatePersonalizedRecommendations ;
    sw:term_status "accepted"@en .

dpv:Credit a rdfs:Class ;
    rdfs:label "Credit"@en ;
    dct:created "2019-04-04"^^xsd:date ;
    dct:creator "Elmar Kiesling; Harshvardhan J. Pandit"^^xsd:string,
        "Fajar Ekaputra"^^xsd:string ;
    dct:date-accepted "2019-06-04"^^xsd:date ;
    dct:description "Information about an individual’s reputation with regards to money"@en ;
    rdfs:isDefinedBy <https://enterprivacy.com/wp-content/uploads/2018/09/Categories-of-Personal-Information.pdf> ;
    rdfs:subClassOf dpv:Financial,
        dpv:Transactional ;
    sw:term_status "accepted"@en .

dpv:CreditCapacity a rdfs:Class ;
    rdfs:label "Credit Capacity"@en ;
    dct:created "2019-04-04"^^xsd:date ;
    dct:creator "Elmar Kiesling; Harshvardhan J. Pandit"^^xsd:string,
        "Fajar Ekaputra"^^xsd:string ;
    dct:date-accepted "2019-06-04"^^xsd:date ;
    dct:description "Information relating to an individual's credit capacity."@en ;
    rdfs:isDefinedBy <https://enterprivacy.com/wp-content/uploads/2018/09/Categories-of-Personal-Information.pdf> ;
    rdfs:subClassOf dpv:Credit ;
    sw:term_status "accepted"@en .

dpv:CreditCardNumber a rdfs:Class ;
    rdfs:label "Credit Card Number"@en ;
    dct:created "2019-04-04"^^xsd:date ;
    dct:creator "Elmar Kiesling; Harshvardhan J. Pandit"^^xsd:string,
        "Fajar Ekaputra"^^xsd:string ;
    dct:date-accepted "2019-06-04"^^xsd:date ;
    dct:description "Information about an individual's credit card number"@en ;
    rdfs:isDefinedBy <https://enterprivacy.com/wp-content/uploads/2018/09/Categories-of-Personal-Information.pdf> ;
    rdfs:subClassOf dpv:AccountIdentifier ;
    sw:term_status "accepted"@en .

dpv:CreditRecord a rdfs:Class ;
    rdfs:label "Credit Record"@en ;
    dct:created "2019-04-04"^^xsd:date ;
    dct:creator "Elmar Kiesling; Harshvardhan J. Pandit"^^xsd:string,
        "Fajar Ekaputra"^^xsd:string ;
    dct:date-accepted "2019-06-04"^^xsd:date ;
    dct:description "Information relating to an individual's credit record."@en ;
    rdfs:isDefinedBy <https://enterprivacy.com/wp-content/uploads/2018/09/Categories-of-Personal-Information.pdf> ;
    rdfs:subClassOf dpv:Credit ;
    sw:term_status "accepted"@en .

dpv:CreditScore a rdfs:Class ;
    rdfs:label "Credit Score"@en ;
    dct:created "2019-04-04"^^xsd:date ;
    dct:creator "Elmar Kiesling; Harshvardhan J. Pandit"^^xsd:string,
        "Fajar Ekaputra"^^xsd:string ;
    dct:date-accepted "2019-06-04"^^xsd:date ;
    dct:description "Information relating to an individual's credit score."@en ;
    rdfs:isDefinedBy <https://enterprivacy.com/wp-content/uploads/2018/09/Categories-of-Personal-Information.pdf> ;
    rdfs:subClassOf dpv:CreditWorthiness ;
    sw:term_status "accepted"@en .

dpv:CreditStanding a rdfs:Class ;
    rdfs:label "Credit Standing"@en ;
    dct:created "2019-04-04"^^xsd:date ;
    dct:creator "Elmar Kiesling; Harshvardhan J. Pandit"^^xsd:string,
        "Fajar Ekaputra"^^xsd:string ;
    dct:date-accepted "2019-06-04"^^xsd:date ;
    dct:description "Information relating to an individual's credit standing."@en ;
    rdfs:isDefinedBy <https://enterprivacy.com/wp-content/uploads/2018/09/Categories-of-Personal-Information.pdf> ;
    rdfs:subClassOf dpv:Credit ;
    sw:term_status "accepted"@en .

dpv:CreditWorthiness a rdfs:Class ;
    rdfs:label "Credit Worthiness"@en ;
    dct:created "2019-04-04"^^xsd:date ;
    dct:creator "Elmar Kiesling; Harshvardhan J. Pandit"^^xsd:string,
        "Fajar Ekaputra"^^xsd:string ;
    dct:date-accepted "2019-06-04"^^xsd:date ;
    dct:description "Information relating to an individual's credit worthiness."@en ;
    rdfs:isDefinedBy <https://enterprivacy.com/wp-content/uploads/2018/09/Categories-of-Personal-Information.pdf> ;
    rdfs:subClassOf dpv:Credit ;
    sw:term_status "accepted"@en .

dpv:Criminal a rdfs:Class ;
    rdfs:label "Criminal"@en ;
    dct:created "2019-04-04"^^xsd:date ;
    dct:creator "Elmar Kiesling; Harshvardhan J. Pandit"^^xsd:string,
        "Fajar Ekaputra"^^xsd:string ;
    dct:date-accepted "2019-06-04"^^xsd:date ;
    dct:description "Information about an individual’s criminal activity e.g. criminal convictions or jail time"@en ;
    rdfs:isDefinedBy <https://enterprivacy.com/wp-content/uploads/2018/09/Categories-of-Personal-Information.pdf> ;
    rdfs:seeAlso svd:Judicial ;
    rdfs:subClassOf dpv:Social ;
    sw:term_status "accepted"@en .

dpv:CriminalCharge a rdfs:Class ;
    rdfs:label "Criminal Charge"@en ;
    dct:created "2019-04-04"^^xsd:date ;
    dct:creator "Elmar Kiesling; Harshvardhan J. Pandit"^^xsd:string,
        "Fajar Ekaputra"^^xsd:string ;
    dct:date-accepted "2019-06-04"^^xsd:date ;
    dct:description "Information on an individual's criminal charges."@en ;
    rdfs:isDefinedBy <https://enterprivacy.com/wp-content/uploads/2018/09/Categories-of-Personal-Information.pdf> ;
    rdfs:subClassOf dpv:Criminal ;
    sw:term_status "accepted"@en .

dpv:CriminalConviction a rdfs:Class ;
    rdfs:label "Criminal Conviction"@en ;
    dct:created "2019-04-04"^^xsd:date ;
    dct:creator "Elmar Kiesling; Harshvardhan J. Pandit"^^xsd:string,
        "Fajar Ekaputra"^^xsd:string ;
    dct:date-accepted "2019-06-04"^^xsd:date ;
    dct:description "Information on an individual's criminal convictions."@en ;
    rdfs:isDefinedBy <https://enterprivacy.com/wp-content/uploads/2018/09/Categories-of-Personal-Information.pdf> ;
    rdfs:subClassOf dpv:Criminal ;
    sw:term_status "accepted"@en .

dpv:CriminalPardon a rdfs:Class ;
    rdfs:label "Criminal Pardon"@en ;
    dct:created "2019-04-04"^^xsd:date ;
    dct:creator "Elmar Kiesling; Harshvardhan J. Pandit"^^xsd:string,
        "Fajar Ekaputra"^^xsd:string ;
    dct:date-accepted "2019-06-04"^^xsd:date ;
    dct:description "Information on an individual's criminal pardons."@en ;
    rdfs:isDefinedBy <https://enterprivacy.com/wp-content/uploads/2018/09/Categories-of-Personal-Information.pdf> ;
    rdfs:subClassOf dpv:Criminal ;
    sw:term_status "accepted"@en .

dpv:CustomerCare a rdfs:Class ;
    rdfs:label "Customer Care"@en ;
    dct:created "2018-12-10"^^xsd:date ;
    dct:creator "Axel Polleres"^^xsd:string,
        "Elmar Kiesling"^^xsd:string,
        "Fajar Ekaputra"^^xsd:string,
        "Harshvardhan J. Pandit"^^xsd:string,
        "Javier Fernandez"^^xsd:string,
        "Simon Steyskal"^^xsd:string ;
    dct:date-accepted "2019-04-05"^^xsd:date ;
    dct:description "Processes related to providing assistance for customer satisfaction"@en ;
    rdfs:isDefinedBy <https://www.w3.org/community/dpvcg/wiki/Purposes_for_handling_Personal_Data#High-level_categories_.28to-be-discussed.29> ;
    rdfs:seeAlso svpu:Feedback ;
    rdfs:subClassOf dpv:ServiceProvision ;
    sw:term_status "accepted"@en .

dpv:CustomerRelationshipManagement a rdfs:Class ;
    rdfs:label "Customer Relationship Management"@en ;
    dct:created "2020-07-08"^^xsd:date ;
    dct:creator "Beatriz"^^xsd:string,
        "Georg"^^xsd:string,
        "Harsh"^^xsd:string ;
    dct:description "Process by which a company can manage and analyse its own interactions with its past, current and potential customers"@en ;
    sw:term_status "proposed"@en .

dpv:DNACode a rdfs:Class ;
    rdfs:label "DNA Code"@en ;
    dct:created "2019-04-04"^^xsd:date ;
    dct:creator "Elmar Kiesling; Harshvardhan J. Pandit"^^xsd:string,
        "Fajar Ekaputra"^^xsd:string ;
    dct:date-accepted "2019-06-04"^^xsd:date ;
    dct:description "Information about an individual's DNA."@en ;
    rdfs:isDefinedBy <https://enterprivacy.com/wp-content/uploads/2018/09/Categories-of-Personal-Information.pdf> ;
    rdfs:subClassOf dpv:MedicalHealth ;
    sw:term_status "accepted"@en .

dpv:DataController a rdfs:Class ;
    rdfs:label "Data Controller"@en ;
    dct:created "2019-04-04"^^xsd:date ;
    dct:creator "Axel Polleres"^^xsd:string,
        "Javier Ferenandez"^^xsd:string ;
    dct:date-accepted "2019-04-05"^^xsd:date ;
    dct:description "The class of Data Controllers that control this particular data handling, any legal entity that is defined by article 4.7 of GDPR."@en ;
    rdfs:isDefinedBy <https://eur-lex.europa.eu/eli/reg/2016/679/art_4/par_7/pnt_g/oj> ;
    sw:term_status "accepted"@en .

dpv:DataProcessor a rdfs:Class ;
    rdfs:label "Data Processor"@en ;
    dct:created "2019-06-04"^^xsd:date ;
    dct:creator "Harshvardhan J. Pandit"^^xsd:string ;
    dct:date-accepted "2019-06-04"^^xsd:date ;
    dct:description "‘processor’ means a natural or legal person, public authority, agency or other body which processes personal data on behalf of the controller;"@en ;
    rdfs:isDefinedBy <https://eur-lex.europa.eu/eli/reg/2016/679/art_4/par_8/pnt_g/oj> ;
    rdfs:subClassOf dpv:Recipient ;
    sw:term_status "accepted"@en .

dpv:DataSource a rdfs:Class ;
    rdfs:label "Data Source"@en ;
    dct:created "2020-07-08"^^xsd:date ;
    dct:creator "Beatriz"^^xsd:string,
        "Georg"^^xsd:string,
        "Harsh"^^xsd:string ;
    dct:description "Source of data"@en ;
    rdfs:comment "Source is direct point of data collection; 'origin' would indicate the original/others points of where the data originates from"@en ;
    rdfs:isDefinedBy "DPVCG"^^xsd:string ;
    sw:term_status "proposed"@en .

dpv:DataSubProcessor a rdfs:Class ;
    rdfs:label "Data Sub-Processor"@en ;
    dct:created "2019-06-04"^^xsd:date ;
    dct:creator "Harshvardhan J. Pandit"^^xsd:string ;
    dct:description "A processor engaged by another processor"@en ;
    rdfs:isDefinedBy <https://eur-lex.europa.eu/eli/reg/2016/679/art_28/par_2/pnt_g/oj> ;
    rdfs:subClassOf dpv:DataProcessor ;
    sw:term_status "proposed"@en .

dpv:DataSubject a rdfs:Class ;
    rdfs:label "Data Subject"@en ;
    dct:created "2019-04-04"^^xsd:date ;
    dct:creator "Axel Polleres"^^xsd:string,
        "Javier Ferenandez"^^xsd:string ;
    dct:date-accepted "2019-04-05"^^xsd:date ;
    dct:description "The class of Data Subject that this particular data handling applies to, any legal entity that is defined by article 4.1 of GDPR."@en ;
    rdfs:comment "The alternative to bind a user or role of users to a policy could be to have a special property \"hasPersonalDataHandling\""@en ;
    rdfs:isDefinedBy <https://eur-lex.europa.eu/eli/reg/2016/679/art_4/par_1/pnt_g/oj> ;
    sw:term_status "accepted"@en .

dpv:DeIdentification a rdfs:Class ;
    rdfs:label "De-Identification"@en ;
    dct:created "2019-04-04"^^xsd:date ;
    dct:creator "Axel Polleres"^^xsd:string,
        "Harshvardhan J. Pandit"^^xsd:string,
        "Mark Lizar"^^xsd:string,
        "Rob Brennan"^^xsd:string ;
    dct:date-accepted "2019-04-05"^^xsd:date ;
    dct:description "Process by identifiable personal data (PII) is converted to un-identifiable personal data"@en ;
    rdfs:isDefinedBy "DPVCG"^^xsd:string ;
    rdfs:subClassOf dpv:PseudoAnonymization ;
    sw:term_status "accepted"@en .

dpv:DeliveryOfGoods a rdfs:Class ;
    rdfs:label "Delivery of Goods"@en ;
    dct:created "2018-12-10"^^xsd:date ;
    dct:creator "Axel Polleres"^^xsd:string,
        "Elmar Kiesling"^^xsd:string,
        "Fajar Ekaputra"^^xsd:string,
        "Harshvardhan J. Pandit"^^xsd:string,
        "Javier Fernandez"^^xsd:string,
        "Simon Steyskal"^^xsd:string ;
    dct:date-accepted "2019-04-05"^^xsd:date ;
    dct:description "To deliver goods and services"@en ;
    rdfs:isDefinedBy <https://www.w3.org/community/dpvcg/wiki/Purposes_for_handling_Personal_Data#High-level_categories_.28to-be-discussed.29> ;
    rdfs:seeAlso svpu:Delivery ;
    rdfs:subClassOf dpv:ServiceProvision ;
    sw:term_status "accepted"@en .

dpv:Demeanor a rdfs:Class ;
    rdfs:label "Demeanor"@en ;
    dct:created "2019-04-04"^^xsd:date ;
    dct:creator "Elmar Kiesling; Harshvardhan J. Pandit"^^xsd:string,
        "Fajar Ekaputra"^^xsd:string ;
    dct:date-accepted "2019-06-04"^^xsd:date ;
    dct:description "Information that relates to an individual's demeanor."@en ;
    rdfs:isDefinedBy <https://enterprivacy.com/wp-content/uploads/2018/09/Categories-of-Personal-Information.pdf> ;
    rdfs:subClassOf dpv:Behavioral ;
    sw:term_status "accepted"@en .

dpv:Demographic a rdfs:Class ;
    rdfs:label "Demographic"@en ;
    dct:created "2019-04-04"^^xsd:date ;
    dct:creator "Elmar Kiesling; Harshvardhan J. Pandit"^^xsd:string,
        "Fajar Ekaputra"^^xsd:string ;
    dct:date-accepted "2019-06-04"^^xsd:date ;
    dct:description "Information that describes an individual’s characteristics shared with others"@en ;
    rdfs:isDefinedBy <https://enterprivacy.com/wp-content/uploads/2018/09/Categories-of-Personal-Information.pdf> ;
    rdfs:subClassOf dpv:External ;
    sw:term_status "accepted"@en .

dpv:Derive a rdfs:Class ;
    rdfs:label "Derive"@en ;
    dct:created "2019-04-04"^^xsd:date ;
    dct:date-accepted "2019-05-07"^^xsd:date ;
    dct:description "to create new derivative data from the original data"@en ;
    rdfs:isDefinedBy <https://www.specialprivacy.eu/vocabs/processing> ;
    rdfs:seeAlso svpr:Derive ;
    rdfs:subClassOf dpv:Transform ;
    sw:term_status "accepted"@en .

dpv:DerivedPersonalData a rdfs:Class ;
    rdfs:label "Derived Personal Data"@en ;
    dct:created "2019-05-07"^^xsd:date ;
    dct:creator "Elmar Kiesling; Harshvardhan J. Pandit"^^xsd:string,
        "Fajar Ekaputra"^^xsd:string ;
    dct:date-accepted "2019-05-07"^^xsd:date ;
    dct:description "Derived data is data that has not been directly provided by the DataSubject, but has been derived from other collected or externally obtained data."@en ;
    rdfs:seeAlso svd:Derived ;
    rdfs:subClassOf dpv:PersonalDataCategory ;
    sw:term_status "accepted"@en .

dpv:DesignStandard a rdfs:Class ;
    rdfs:label "Design Standard"@en ;
    dct:created "2019-04-04"^^xsd:date ;
    dct:creator "Axel Polleres"^^xsd:string,
        "Harshvardhan J. Pandit"^^xsd:string,
        "Mark Lizar"^^xsd:string,
        "Rob Brennan"^^xsd:string ;
    dct:date-accepted "2019-04-05"^^xsd:date ;
    dct:description "A set of rules or guidelines outlining criterias for design"@en ;
    rdfs:isDefinedBy "DPVCG"^^xsd:string ;
    rdfs:subClassOf dpv:GuidelinesPrinciple ;
    sw:term_status "accepted"@en .

dpv:Destruct a rdfs:Class ;
    rdfs:label "Destruct"@en ;
    dct:created "2019-04-04"^^xsd:date ;
    dct:date-accepted "2019-05-07"^^xsd:date ;
    dct:description "to process data in a way it no longer exists or cannot be repaired"@en ;
    rdfs:isDefinedBy <https://eur-lex.europa.eu/eli/reg/2016/679/art_4/par_2/oj> ;
    rdfs:subClassOf dpv:Remove ;
    sw:term_status "accepted"@en .

dpv:DeviceBased a rdfs:Class ;
    rdfs:label "Device Based"@en ;
    dct:created "2019-04-04"^^xsd:date ;
    dct:creator "Elmar Kiesling; Harshvardhan J. Pandit"^^xsd:string,
        "Fajar Ekaputra"^^xsd:string ;
    dct:date-accepted "2019-06-04"^^xsd:date ;
    dct:description "Information about a device that an individual uses for personal use (even part-time or with others)"@en ;
    rdfs:isDefinedBy <https://enterprivacy.com/wp-content/uploads/2018/09/Categories-of-Personal-Information.pdf> ;
    rdfs:seeAlso svd:Computer ;
    rdfs:subClassOf dpv:Tracking ;
    sw:term_status "accepted"@en .

dpv:Dialect a rdfs:Class ;
    rdfs:label "Dialect"@en ;
    dct:created "2019-04-04"^^xsd:date ;
    dct:creator "Elmar Kiesling; Harshvardhan J. Pandit"^^xsd:string,
        "Fajar Ekaputra"^^xsd:string ;
    dct:date-accepted "2019-06-04"^^xsd:date ;
    dct:description "Information about an individual’s dialect."@en ;
    rdfs:isDefinedBy <https://enterprivacy.com/wp-content/uploads/2018/09/Categories-of-Personal-Information.pdf> ;
    rdfs:subClassOf dpv:Language ;
    sw:term_status "accepted"@en .

dpv:Disability a rdfs:Class ;
    rdfs:label "Disability"@en ;
    dct:created "2019-04-04"^^xsd:date ;
    dct:creator "Elmar Kiesling; Harshvardhan J. Pandit"^^xsd:string,
        "Fajar Ekaputra"^^xsd:string ;
    dct:date-accepted "2019-06-04"^^xsd:date ;
    dct:description "Information about an individual's disabilities."@en ;
    rdfs:isDefinedBy <https://enterprivacy.com/wp-content/uploads/2018/09/Categories-of-Personal-Information.pdf> ;
    rdfs:subClassOf dpv:MedicalHealth ;
    sw:term_status "accepted"@en .

dpv:DisciplinaryAction a rdfs:Class ;
    rdfs:label "Disciplinary Action"@en ;
    dct:created "2019-04-04"^^xsd:date ;
    dct:creator "Elmar Kiesling; Harshvardhan J. Pandit"^^xsd:string,
        "Fajar Ekaputra"^^xsd:string ;
    dct:date-accepted "2019-06-04"^^xsd:date ;
    dct:description "Information about disciplinary actions associated with an individual"@en ;
    rdfs:isDefinedBy <https://enterprivacy.com/wp-content/uploads/2018/09/Categories-of-Personal-Information.pdf> ;
    rdfs:subClassOf dpv:Professional ;
    sw:term_status "accepted"@en .

dpv:Disclose a rdfs:Class ;
    rdfs:label "Disclose"@en ;
    dct:created "2019-04-04"^^xsd:date ;
    dct:date-accepted "2019-05-07"^^xsd:date ;
    dct:description "to make data known"@en ;
    rdfs:isDefinedBy "DPVCG"^^xsd:string ;
    rdfs:subClassOf dpv:Processing ;
    sw:term_status "accepted"@en .

dpv:DiscloseByTransmission a rdfs:Class ;
    rdfs:label "Disclose by Transmission"@en ;
    dct:created "2019-04-04"^^xsd:date ;
    dct:date-accepted "2019-05-07"^^xsd:date ;
    dct:description "to disclose data by means of transmission"@en ;
    rdfs:isDefinedBy <https://eur-lex.europa.eu/eli/reg/2016/679/art_4/par_2/oj> ;
    rdfs:subClassOf dpv:Disclose ;
    sw:term_status "accepted"@en .

dpv:Dislike a rdfs:Class ;
    rdfs:label "Dislike"@en ;
    dct:created "2019-04-04"^^xsd:date ;
    dct:creator "Elmar Kiesling; Harshvardhan J. Pandit"^^xsd:string,
        "Fajar Ekaputra"^^xsd:string ;
    dct:date-accepted "2019-06-04"^^xsd:date ;
    dct:description "Information relating to a user's dislikes."@en ;
    rdfs:isDefinedBy <https://enterprivacy.com/wp-content/uploads/2018/09/Categories-of-Personal-Information.pdf> ;
    rdfs:subClassOf dpv:Interest ;
    sw:term_status "accepted"@en .

dpv:Disseminate a rdfs:Class ;
    rdfs:label "Disseminate"@en ;
    dct:created "2019-04-04"^^xsd:date ;
    dct:date-accepted "2019-05-07"^^xsd:date ;
    dct:description "to spread data throughout"@en ;
    rdfs:isDefinedBy <https://eur-lex.europa.eu/eli/reg/2016/679/art_4/par_2/oj> ;
    rdfs:subClassOf dpv:Disclose ;
    sw:term_status "accepted"@en .

dpv:Divorce a rdfs:Class ;
    rdfs:label "Divorce"@en ;
    dct:created "2019-04-04"^^xsd:date ;
    dct:creator "Elmar Kiesling; Harshvardhan J. Pandit"^^xsd:string,
        "Fajar Ekaputra"^^xsd:string ;
    dct:date-accepted "2019-06-04"^^xsd:date ;
    dct:description "Information about an individual's divorce(s)."@en ;
    rdfs:isDefinedBy <https://enterprivacy.com/wp-content/uploads/2018/09/Categories-of-Personal-Information.pdf> ;
    rdfs:subClassOf dpv:FamilyStructure ;
    sw:term_status "accepted"@en .

dpv:DrugTestResult a rdfs:Class ;
    rdfs:label "Drug Test Result"@en ;
    dct:created "2019-04-04"^^xsd:date ;
    dct:creator "Elmar Kiesling; Harshvardhan J. Pandit"^^xsd:string,
        "Fajar Ekaputra"^^xsd:string ;
    dct:date-accepted "2019-06-04"^^xsd:date ;
    dct:description "Information about an individual's drug test results."@en ;
    rdfs:isDefinedBy <https://enterprivacy.com/wp-content/uploads/2018/09/Categories-of-Personal-Information.pdf> ;
    rdfs:subClassOf dpv:MedicalHealth ;
    sw:term_status "accepted"@en .

dpv:EmailAddress a rdfs:Class ;
    rdfs:label "Email Address"@en ;
    dct:created "2019-04-04"^^xsd:date ;
    dct:creator "Elmar Kiesling; Harshvardhan J. Pandit"^^xsd:string,
        "Fajar Ekaputra"^^xsd:string ;
    dct:date-accepted "2019-06-04"^^xsd:date ;
    dct:description "Information about an individual's Email address."@en ;
    rdfs:isDefinedBy <https://enterprivacy.com/wp-content/uploads/2018/09/Categories-of-Personal-Information.pdf> ;
    rdfs:subClassOf dpv:Contact ;
    sw:term_status "accepted"@en .

dpv:EmailContent a rdfs:Class ;
    rdfs:label "Email Content"@en ;
    dct:created "2019-04-04"^^xsd:date ;
    dct:creator "Elmar Kiesling; Harshvardhan J. Pandit"^^xsd:string,
        "Fajar Ekaputra"^^xsd:string ;
    dct:date-accepted "2019-06-04"^^xsd:date ;
    dct:description "The contents of Emails that an individual sends or receives."@en ;
    rdfs:isDefinedBy <https://enterprivacy.com/wp-content/uploads/2018/09/Categories-of-Personal-Information.pdf> ;
    rdfs:subClassOf dpv:Communication ;
    sw:term_status "accepted"@en .

dpv:EmploymentHistory a rdfs:Class ;
    rdfs:label "Employment History"@en ;
    dct:created "2019-04-04"^^xsd:date ;
    dct:creator "Elmar Kiesling; Harshvardhan J. Pandit"^^xsd:string,
        "Fajar Ekaputra"^^xsd:string ;
    dct:date-accepted "2019-06-04"^^xsd:date ;
    dct:description "Information about an individual's employment history"@en ;
    rdfs:isDefinedBy <https://enterprivacy.com/wp-content/uploads/2018/09/Categories-of-Personal-Information.pdf> ;
    rdfs:subClassOf dpv:Professional ;
    sw:term_status "accepted"@en .

dpv:EncryptionInRest a rdfs:Class ;
    rdfs:label "Encryption in Rest"@en ;
    dct:created "2019-04-04"^^xsd:date ;
    dct:creator "Axel Polleres"^^xsd:string,
        "Harshvardhan J. Pandit"^^xsd:string,
        "Mark Lizar"^^xsd:string,
        "Rob Brennan"^^xsd:string ;
    dct:date-accepted "2019-04-05"^^xsd:date ;
    dct:description "Encryption of data when being stored (persistent encryption)"@en ;
    rdfs:isDefinedBy "DPVCG"^^xsd:string ;
    rdfs:subClassOf dpv:PseudonymisationEncryption ;
    sw:term_status "accepted"@en .

dpv:EncryptionInTransfer a rdfs:Class ;
    rdfs:label "Encryption in Transfer"@en ;
    dct:created "2019-04-04"^^xsd:date ;
    dct:creator "Axel Polleres"^^xsd:string,
        "Harshvardhan J. Pandit"^^xsd:string,
        "Mark Lizar"^^xsd:string,
        "Rob Brennan"^^xsd:string ;
    dct:date-accepted "2019-04-05"^^xsd:date ;
    dct:description "Encryption of data in transit e.g. when being transferred from one location to another, including sharing"@en ;
    rdfs:isDefinedBy "DPVCG"^^xsd:string ;
    rdfs:subClassOf dpv:PseudonymisationEncryption ;
    sw:term_status "accepted"@en .

dpv:Erase a rdfs:Class ;
    rdfs:label "Erase"@en ;
    dct:created "2019-04-04"^^xsd:date ;
    dct:date-accepted "2019-05-07"^^xsd:date ;
    dct:description "to delete data"@en ;
    rdfs:isDefinedBy <https://eur-lex.europa.eu/eli/reg/2016/679/art_4/par_2/oj> ;
    rdfs:subClassOf dpv:Remove ;
    sw:term_status "accepted"@en .

dpv:EthnicOrigin a rdfs:Class ;
    rdfs:label "Ethnic Origin"@en ;
    dct:created "2019-04-04"^^xsd:date ;
    dct:creator "Elmar Kiesling; Harshvardhan J. Pandit"^^xsd:string,
        "Fajar Ekaputra"^^xsd:string ;
    dct:date-accepted "2019-06-04"^^xsd:date ;
    dct:description "Information related to an individual's ethnic origin."@en ;
    rdfs:isDefinedBy <https://enterprivacy.com/wp-content/uploads/2018/09/Categories-of-Personal-Information.pdf> ;
    rdfs:subClassOf dpv:Ethnicity,
        dpv:SpecialCategoryPersonalData ;
    sw:term_status "accepted"@en .

dpv:Ethnicity a rdfs:Class ;
    rdfs:label "Ethnicity"@en ;
    dct:created "2019-04-04"^^xsd:date ;
    dct:creator "Elmar Kiesling; Harshvardhan J. Pandit"^^xsd:string,
        "Fajar Ekaputra"^^xsd:string ;
    dct:date-accepted "2019-06-04"^^xsd:date ;
    dct:description "Information that describes an individual’s origins and lineage"@en ;
    rdfs:isDefinedBy <https://enterprivacy.com/wp-content/uploads/2018/09/Categories-of-Personal-Information.pdf> ;
    rdfs:subClassOf dpv:External ;
    sw:term_status "accepted"@en .

dpv:External a rdfs:Class ;
    rdfs:label "External"@en ;
    dct:created "2019-04-04"^^xsd:date ;
    dct:creator "Elmar Kiesling; Harshvardhan J. Pandit"^^xsd:string,
        "Fajar Ekaputra"^^xsd:string ;
    dct:date-accepted "2019-06-04"^^xsd:date ;
    dct:description "Personal Data that can be observed by another person i.e. has external characteristics that make it visible"@en ;
    rdfs:isDefinedBy <https://enterprivacy.com/wp-content/uploads/2018/09/Categories-of-Personal-Information.pdf> ;
    rdfs:subClassOf dpv:PersonalDataCategory ;
    sw:term_status "accepted"@en .

dpv:Family a rdfs:Class ;
    rdfs:label "Family"@en ;
    dct:created "2019-04-04"^^xsd:date ;
    dct:creator "Elmar Kiesling; Harshvardhan J. Pandit"^^xsd:string,
        "Fajar Ekaputra"^^xsd:string ;
    dct:date-accepted "2019-06-04"^^xsd:date ;
    dct:description "Information about an individual’s family and relationships"@en ;
    rdfs:isDefinedBy <https://enterprivacy.com/wp-content/uploads/2018/09/Categories-of-Personal-Information.pdf> ;
    rdfs:subClassOf dpv:Social ;
    sw:term_status "accepted"@en .

dpv:FamilyHealthHistory a rdfs:Class ;
    rdfs:label "Family Health History"@en ;
    dct:created "2019-04-04"^^xsd:date ;
    dct:creator "Elmar Kiesling; Harshvardhan J. Pandit"^^xsd:string,
        "Fajar Ekaputra"^^xsd:string ;
    dct:date-accepted "2019-06-04"^^xsd:date ;
    dct:description "Information related to an individual's family health history."@en ;
    rdfs:isDefinedBy <https://enterprivacy.com/wp-content/uploads/2018/09/Categories-of-Personal-Information.pdf> ;
    rdfs:subClassOf dpv:HealthHistory ;
    sw:term_status "accepted"@en .

dpv:FamilyStructure a rdfs:Class ;
    rdfs:label "Family Structure"@en ;
    dct:created "2019-04-04"^^xsd:date ;
    dct:creator "Elmar Kiesling; Harshvardhan J. Pandit"^^xsd:string,
        "Fajar Ekaputra"^^xsd:string ;
    dct:date-accepted "2019-06-04"^^xsd:date ;
    dct:description "Information that describes an individual's family structure."@en ;
    rdfs:isDefinedBy <https://enterprivacy.com/wp-content/uploads/2018/09/Categories-of-Personal-Information.pdf> ;
    rdfs:subClassOf dpv:Family ;
    sw:term_status "accepted"@en .

dpv:Favorite a rdfs:Class ;
    rdfs:label "Favorite"@en ;
    dct:created "2019-04-04"^^xsd:date ;
    dct:creator "Elmar Kiesling; Harshvardhan J. Pandit"^^xsd:string,
        "Fajar Ekaputra"^^xsd:string ;
    dct:date-accepted "2019-06-04"^^xsd:date ;
    dct:description "Information about an individual's favorites"@en ;
    rdfs:isDefinedBy <https://enterprivacy.com/wp-content/uploads/2018/09/Categories-of-Personal-Information.pdf> ;
    rdfs:subClassOf dpv:Preference ;
    sw:term_status "accepted"@en .

dpv:FavoriteColor a rdfs:Class ;
    rdfs:label "Favorite Color"@en ;
    dct:created "2019-04-04"^^xsd:date ;
    dct:creator "Elmar Kiesling; Harshvardhan J. Pandit"^^xsd:string,
        "Fajar Ekaputra"^^xsd:string ;
    dct:date-accepted "2019-06-04"^^xsd:date ;
    dct:description "Information about an individual's favorite color."@en ;
    rdfs:isDefinedBy <https://enterprivacy.com/wp-content/uploads/2018/09/Categories-of-Personal-Information.pdf> ;
    rdfs:subClassOf dpv:Favorite ;
    sw:term_status "accepted"@en .

dpv:FavoriteFood a rdfs:Class ;
    rdfs:label "Favorite Food"@en ;
    dct:created "2019-04-04"^^xsd:date ;
    dct:creator "Elmar Kiesling; Harshvardhan J. Pandit"^^xsd:string,
        "Fajar Ekaputra"^^xsd:string ;
    dct:date-accepted "2019-06-04"^^xsd:date ;
    dct:description "Information about an individual's favorite food."@en ;
    rdfs:isDefinedBy <https://enterprivacy.com/wp-content/uploads/2018/09/Categories-of-Personal-Information.pdf> ;
    rdfs:subClassOf dpv:Favorite ;
    sw:term_status "accepted"@en .

dpv:FavoriteMusic a rdfs:Class ;
    rdfs:label "Favorite Music"@en ;
    dct:created "2019-04-04"^^xsd:date ;
    dct:creator "Elmar Kiesling; Harshvardhan J. Pandit"^^xsd:string,
        "Fajar Ekaputra"^^xsd:string ;
    dct:date-accepted "2019-06-04"^^xsd:date ;
    dct:description "Information about an individual's favorite music."@en ;
    rdfs:isDefinedBy <https://enterprivacy.com/wp-content/uploads/2018/09/Categories-of-Personal-Information.pdf> ;
    rdfs:subClassOf dpv:Favorite ;
    sw:term_status "accepted"@en .

dpv:Fetish a rdfs:Class ;
    rdfs:label "Fetish"@en ;
    dct:created "2019-04-04"^^xsd:date ;
    dct:creator "Elmar Kiesling; Harshvardhan J. Pandit"^^xsd:string,
        "Fajar Ekaputra"^^xsd:string ;
    dct:date-accepted "2019-06-04"^^xsd:date ;
    dct:description "Information an individual's sexual fetishes"@en ;
    rdfs:isDefinedBy <https://enterprivacy.com/wp-content/uploads/2018/09/Categories-of-Personal-Information.pdf> ;
    rdfs:subClassOf dpv:Sexual ;
    sw:term_status "accepted"@en .

dpv:Financial a rdfs:Class ;
    rdfs:label "Financial"@en ;
    dct:created "2019-04-04"^^xsd:date ;
    dct:creator "Elmar Kiesling; Harshvardhan J. Pandit"^^xsd:string,
        "Fajar Ekaputra"^^xsd:string ;
    dct:date-accepted "2019-06-04"^^xsd:date ;
    dct:description "Personal data regarding finance or monetary information"@en ;
    rdfs:isDefinedBy <https://enterprivacy.com/wp-content/uploads/2018/09/Categories-of-Personal-Information.pdf> ;
    rdfs:seeAlso svd:Financial ;
    rdfs:subClassOf dpv:PersonalDataCategory ;
    sw:term_status "accepted"@en .

dpv:FinancialAccount a rdfs:Class ;
    rdfs:label "Financial Account"@en ;
    dct:created "2019-04-04"^^xsd:date ;
    dct:creator "Elmar Kiesling; Harshvardhan J. Pandit"^^xsd:string,
        "Fajar Ekaputra"^^xsd:string ;
    dct:date-accepted "2019-06-04"^^xsd:date ;
    dct:description "Information that identifies an individual’s financial account"@en ;
    rdfs:isDefinedBy <https://enterprivacy.com/wp-content/uploads/2018/09/Categories-of-Personal-Information.pdf> ;
    rdfs:subClassOf dpv:Financial ;
    sw:term_status "accepted"@en .

dpv:FinancialAccountNumber a rdfs:Class ;
    rdfs:label "Financial Account Number"@en ;
    dct:created "2019-04-04"^^xsd:date ;
    dct:creator "Elmar Kiesling; Harshvardhan J. Pandit"^^xsd:string,
        "Fajar Ekaputra"^^xsd:string ;
    dct:date-accepted "2019-06-04"^^xsd:date ;
    dct:description "Information about an individual's financial account number"@en ;
    rdfs:isDefinedBy <https://enterprivacy.com/wp-content/uploads/2018/09/Categories-of-Personal-Information.pdf> ;
    rdfs:subClassOf dpv:AccountIdentifier ;
    sw:term_status "accepted"@en .

dpv:Fingerprint a rdfs:Class ;
    rdfs:label "Fingerprint"@en ;
    dct:created "2019-04-04"^^xsd:date ;
    dct:creator "Elmar Kiesling; Harshvardhan J. Pandit"^^xsd:string,
        "Fajar Ekaputra"^^xsd:string ;
    dct:date-accepted "2019-06-04"^^xsd:date ;
    dct:description "Information related to an individual's fingerprint used for biometric purposes."@en ;
    rdfs:isDefinedBy <https://enterprivacy.com/wp-content/uploads/2018/09/Categories-of-Personal-Information.pdf> ;
    rdfs:subClassOf dpv:Biometric ;
    sw:term_status "accepted"@en .

dpv:FraudPreventionAndDetection a rdfs:Class ;
    rdfs:label "Fraud Prevention and Detection"@en ;
    dct:created "2018-12-10"^^xsd:date ;
    dct:creator "Axel Polleres"^^xsd:string,
        "Elmar Kiesling"^^xsd:string,
        "Fajar Ekaputra"^^xsd:string,
        "Harshvardhan J. Pandit"^^xsd:string,
        "Javier Fernandez"^^xsd:string,
        "Simon Steyskal"^^xsd:string ;
    dct:date-accepted "2019-04-05"^^xsd:date ;
    dct:description "To detect and prevent fraud"@en ;
    rdfs:isDefinedBy <https://www.w3.org/community/dpvcg/wiki/Purposes_for_handling_Personal_Data#High-level_categories_.28to-be-discussed.29> ;
    rdfs:seeAlso svpu:Government ;
    rdfs:subClassOf dpv:Security ;
    sw:term_status "accepted"@en .

dpv:Friend a rdfs:Class ;
    rdfs:label "Friend"@en ;
    dct:created "2019-04-04"^^xsd:date ;
    dct:creator "Elmar Kiesling; Harshvardhan J. Pandit"^^xsd:string,
        "Fajar Ekaputra"^^xsd:string ;
    dct:date-accepted "2019-06-04"^^xsd:date ;
    dct:description "Information about friends of the individual in a social network. Includes aspects of friendships such as years together or nature of friendship."@en ;
    rdfs:isDefinedBy <https://enterprivacy.com/wp-content/uploads/2018/09/Categories-of-Personal-Information.pdf> ;
    rdfs:subClassOf dpv:SocialNetwork ;
    sw:term_status "accepted"@en .

dpv:GPSCoordinate a rdfs:Class ;
    rdfs:label "GPS Coordinate"@en ;
    dct:created "2019-04-04"^^xsd:date ;
    dct:creator "Elmar Kiesling; Harshvardhan J. Pandit"^^xsd:string,
        "Fajar Ekaputra"^^xsd:string ;
    dct:date-accepted "2019-06-04"^^xsd:date ;
    dct:description "Global position system coordinates of a user's location."@en ;
    rdfs:isDefinedBy <https://enterprivacy.com/wp-content/uploads/2018/09/Categories-of-Personal-Information.pdf> ;
    rdfs:subClassOf dpv:Location ;
    sw:term_status "accepted"@en .

dpv:Gender a rdfs:Class ;
    rdfs:label "Gender"@en ;
    dct:created "2019-04-04"^^xsd:date ;
    dct:creator "Elmar Kiesling; Harshvardhan J. Pandit"^^xsd:string,
        "Fajar Ekaputra"^^xsd:string ;
    dct:date-accepted "2019-06-04"^^xsd:date ;
    dct:description "Information about an individual's gender"@en ;
    rdfs:isDefinedBy <https://enterprivacy.com/wp-content/uploads/2018/09/Categories-of-Personal-Information.pdf> ;
    rdfs:subClassOf dpv:PhysicalCharacteristic ;
    sw:term_status "accepted"@en .

dpv:GeneralReputation a rdfs:Class ;
    rdfs:label "General Reputation"@en ;
    dct:created "2019-04-04"^^xsd:date ;
    dct:creator "Elmar Kiesling; Harshvardhan J. Pandit"^^xsd:string,
        "Fajar Ekaputra"^^xsd:string ;
    dct:date-accepted "2019-06-04"^^xsd:date ;
    dct:description "Information about an individual's reputation in the public sphere"@en ;
    rdfs:isDefinedBy <https://enterprivacy.com/wp-content/uploads/2018/09/Categories-of-Personal-Information.pdf> ;
    rdfs:subClassOf dpv:PublicLife ;
    sw:term_status "accepted"@en .

dpv:Geographic a rdfs:Class ;
    rdfs:label "Geographic"@en ;
    dct:created "2019-04-04"^^xsd:date ;
    dct:creator "Elmar Kiesling; Harshvardhan J. Pandit"^^xsd:string,
        "Fajar Ekaputra"^^xsd:string ;
    dct:date-accepted "2019-06-04"^^xsd:date ;
    dct:description "Geographic information relating to an individual (e.g., home address)"@en ;
    rdfs:isDefinedBy <https://enterprivacy.com/wp-content/uploads/2018/09/Categories-of-Personal-Information.pdf> ;
    rdfs:subClassOf dpv:Demographic ;
    sw:term_status "accepted"@en .

dpv:GroupMembership a rdfs:Class ;
    rdfs:label "Group Membership"@en ;
    dct:created "2019-04-04"^^xsd:date ;
    dct:creator "Elmar Kiesling; Harshvardhan J. Pandit"^^xsd:string,
        "Fajar Ekaputra"^^xsd:string ;
    dct:date-accepted "2019-06-04"^^xsd:date ;
    dct:description "Information about groups the individual is included or associated with in a social network"@en ;
    rdfs:isDefinedBy <https://enterprivacy.com/wp-content/uploads/2018/09/Categories-of-Personal-Information.pdf> ;
    rdfs:subClassOf dpv:SocialNetwork ;
    sw:term_status "accepted"@en .

dpv:GuidelinesPrinciple a rdfs:Class ;
    rdfs:label "GuidelinesPrinciple"@en ;
    dct:created "2019-04-04"^^xsd:date ;
    dct:creator "Axel Polleres"^^xsd:string,
        "Harshvardhan J. Pandit"^^xsd:string,
        "Mark Lizar"^^xsd:string,
        "Rob Brennan"^^xsd:string ;
    dct:date-accepted "2019-04-05"^^xsd:date ;
    dct:description "Guidelines or Principles regarding processing and operational measures"@en ;
    rdfs:isDefinedBy "DPVCG"^^xsd:string ;
    rdfs:subClassOf dpv:OrganisationalMeasure ;
    sw:term_status "accepted"@en .

dpv:HairColor a rdfs:Class ;
    rdfs:label "Hair Color"@en ;
    dct:created "2019-04-04"^^xsd:date ;
    dct:creator "Elmar Kiesling; Harshvardhan J. Pandit"^^xsd:string,
        "Fajar Ekaputra"^^xsd:string ;
    dct:date-accepted "2019-06-04"^^xsd:date ;
    dct:description "Information about an individual's hair colour"@en ;
    rdfs:isDefinedBy <https://enterprivacy.com/wp-content/uploads/2018/09/Categories-of-Personal-Information.pdf> ;
    rdfs:subClassOf dpv:PhysicalCharacteristic ;
    sw:term_status "accepted"@en .

dpv:Health a rdfs:Class ;
    rdfs:label "Health"@en ;
    dct:created "2019-04-04"^^xsd:date ;
    dct:creator "Elmar Kiesling; Harshvardhan J. Pandit"^^xsd:string,
        "Fajar Ekaputra"^^xsd:string ;
    dct:date-accepted "2019-06-04"^^xsd:date ;
    dct:description "Information about an individual's health."@en ;
    rdfs:isDefinedBy <https://enterprivacy.com/wp-content/uploads/2018/09/Categories-of-Personal-Information.pdf> ;
    rdfs:seeAlso svd:Health ;
    rdfs:subClassOf dpv:MedicalHealth ;
    sw:term_status "accepted"@en .

dpv:HealthHistory a rdfs:Class ;
    rdfs:label "Health History"@en ;
    dct:created "2019-04-04"^^xsd:date ;
    dct:creator "Elmar Kiesling; Harshvardhan J. Pandit"^^xsd:string,
        "Fajar Ekaputra"^^xsd:string ;
    dct:date-accepted "2019-06-04"^^xsd:date ;
    dct:description "Information about an individual's health history."@en ;
    rdfs:isDefinedBy <https://enterprivacy.com/wp-content/uploads/2018/09/Categories-of-Personal-Information.pdf> ;
    rdfs:subClassOf dpv:MedicalHealth ;
    sw:term_status "accepted"@en .

dpv:HealthRecord a rdfs:Class ;
    rdfs:label "Health Record"@en ;
    dct:created "2019-04-04"^^xsd:date ;
    dct:creator "Elmar Kiesling; Harshvardhan J. Pandit"^^xsd:string,
        "Fajar Ekaputra"^^xsd:string ;
    dct:date-accepted "2019-06-04"^^xsd:date ;
    dct:description "Information about an individual's health record."@en ;
    rdfs:isDefinedBy <https://enterprivacy.com/wp-content/uploads/2018/09/Categories-of-Personal-Information.pdf> ;
    rdfs:subClassOf dpv:MedicalHealth ;
    sw:term_status "accepted"@en .

dpv:Height a rdfs:Class ;
    rdfs:label "Height"@en ;
    dct:created "2019-04-04"^^xsd:date ;
    dct:creator "Elmar Kiesling; Harshvardhan J. Pandit"^^xsd:string,
        "Fajar Ekaputra"^^xsd:string ;
    dct:date-accepted "2019-06-04"^^xsd:date ;
    dct:description "Information about an individual's physical height"@en ;
    rdfs:isDefinedBy <https://enterprivacy.com/wp-content/uploads/2018/09/Categories-of-Personal-Information.pdf> ;
    rdfs:subClassOf dpv:PhysicalCharacteristic ;
    sw:term_status "accepted"@en .

dpv:Historical a rdfs:Class ;
    rdfs:label "Historical"@en ;
    dct:created "2019-04-04"^^xsd:date ;
    dct:creator "Elmar Kiesling; Harshvardhan J. Pandit"^^xsd:string,
        "Fajar Ekaputra"^^xsd:string ;
    dct:date-accepted "2019-06-04"^^xsd:date ;
    dct:description "Historical personal data is that which is related to or relevant for history or past events in the context of the person or their life."@en ;
    rdfs:isDefinedBy <https://enterprivacy.com/wp-content/uploads/2018/09/Categories-of-Personal-Information.pdf> ;
    rdfs:subClassOf dpv:PersonalDataCategory ;
    sw:term_status "accepted"@en .

dpv:HouseOwned a rdfs:Class ;
    rdfs:label "House Owned"@en ;
    dct:created "2019-04-04"^^xsd:date ;
    dct:creator "Elmar Kiesling; Harshvardhan J. Pandit"^^xsd:string,
        "Fajar Ekaputra"^^xsd:string ;
    dct:date-accepted "2019-06-04"^^xsd:date ;
    dct:description "Information about house(s) owned by an individual."@en ;
    rdfs:isDefinedBy <https://enterprivacy.com/wp-content/uploads/2018/09/Categories-of-Personal-Information.pdf> ;
    rdfs:subClassOf dpv:Ownership ;
    sw:term_status "accepted"@en .

dpv:IPAddress a rdfs:Class ;
    rdfs:label "IP Address"@en ;
    dct:created "2019-04-04"^^xsd:date ;
    dct:creator "Elmar Kiesling; Harshvardhan J. Pandit"^^xsd:string,
        "Fajar Ekaputra"^^xsd:string ;
    dct:date-accepted "2019-06-04"^^xsd:date ;
    dct:description "An Internet protocol (IP) address of a device used by an individual."@en ;
    rdfs:isDefinedBy <https://enterprivacy.com/wp-content/uploads/2018/09/Categories-of-Personal-Information.pdf> ;
    rdfs:subClassOf dpv:DeviceBased ;
    sw:term_status "accepted"@en .

dpv:Identifying a rdfs:Class ;
    rdfs:label "Identifying"@en ;
    dct:created "2019-04-04"^^xsd:date ;
    dct:creator "Elmar Kiesling; Harshvardhan J. Pandit"^^xsd:string,
        "Fajar Ekaputra"^^xsd:string ;
    dct:date-accepted "2019-06-04"^^xsd:date ;
    dct:description "Information that uniquely or semi-uniquely identifies a specific individual"@en ;
    rdfs:isDefinedBy <https://enterprivacy.com/wp-content/uploads/2018/09/Categories-of-Personal-Information.pdf> ;
    rdfs:subClassOf dpv:External ;
    sw:term_status "accepted"@en .

dpv:IdentityVerification a rdfs:Class ;
    rdfs:label "Identity Verification"@en ;
    dct:created "2018-12-10"^^xsd:date ;
    dct:creator "Axel Polleres"^^xsd:string,
        "Elmar Kiesling"^^xsd:string,
        "Fajar Ekaputra"^^xsd:string,
        "Harshvardhan J. Pandit"^^xsd:string,
        "Javier Fernandez"^^xsd:string,
        "Simon Steyskal"^^xsd:string ;
    dct:date-accepted "2019-04-05"^^xsd:date ;
    dct:description "To verify and authorise identity"@en ;
    rdfs:isDefinedBy <https://www.w3.org/community/dpvcg/wiki/Purposes_for_handling_Personal_Data#High-level_categories_.28to-be-discussed.29> ;
    rdfs:subClassOf dpv:Security ;
    sw:term_status "accepted"@en .

dpv:ImproveExistingProductsAndServices a rdfs:Class ;
    rdfs:label "Improve Existing Products and Services"@en ;
    dct:created "2018-12-10"^^xsd:date ;
    dct:creator "Axel Polleres"^^xsd:string,
        "Elmar Kiesling"^^xsd:string,
        "Fajar Ekaputra"^^xsd:string,
        "Harshvardhan J. Pandit"^^xsd:string,
        "Javier Fernandez"^^xsd:string,
        "Simon Steyskal"^^xsd:string ;
    dct:date-accepted "2019-04-05"^^xsd:date ;
    dct:description "To improve existing products and services"@en ;
    rdfs:isDefinedBy <https://www.w3.org/community/dpvcg/wiki/Purposes_for_handling_Personal_Data#High-level_categories_.28to-be-discussed.29> ;
    rdfs:subClassOf dpv:OptimisationForController ;
    sw:term_status "accepted"@en .

dpv:ImproveInternalCRMProcesses a rdfs:Class ;
    rdfs:label "Improve Internal CRM Processes"@en ;
    dct:created "2018-12-10"^^xsd:date ;
    dct:creator "Axel Polleres"^^xsd:string,
        "Elmar Kiesling"^^xsd:string,
        "Fajar Ekaputra"^^xsd:string,
        "Harshvardhan J. Pandit"^^xsd:string,
        "Javier Fernandez"^^xsd:string,
        "Simon Steyskal"^^xsd:string ;
    dct:date-accepted "2019-04-05"^^xsd:date ;
    dct:description "To improve customer-relationship management (CRM) processes"@en ;
    rdfs:isDefinedBy <https://www.w3.org/community/dpvcg/wiki/Purposes_for_handling_Personal_Data#High-level_categories_.28to-be-discussed.29> ;
    rdfs:subClassOf dpv:OptimisationForController ;
    sw:term_status "accepted"@en .

dpv:Income a rdfs:Class ;
    rdfs:label "Income"@en ;
    dct:created "2019-04-04"^^xsd:date ;
    dct:creator "Elmar Kiesling; Harshvardhan J. Pandit"^^xsd:string,
        "Fajar Ekaputra"^^xsd:string ;
    dct:date-accepted "2019-06-04"^^xsd:date ;
    dct:description "Information about financial income e.g. for individual or household or family"@en ;
    rdfs:isDefinedBy <https://enterprivacy.com/wp-content/uploads/2018/09/Categories-of-Personal-Information.pdf> ;
    rdfs:subClassOf dpv:Transactional ;
    sw:term_status "accepted"@en .

dpv:IncomeBracket a rdfs:Class ;
    rdfs:label "Income Bracket"@en ;
    dct:created "2019-04-04"^^xsd:date ;
    dct:creator "Elmar Kiesling; Harshvardhan J. Pandit"^^xsd:string,
        "Fajar Ekaputra"^^xsd:string ;
    dct:date-accepted "2019-06-04"^^xsd:date ;
    dct:description "Information about an individual's income bracket."@en ;
    rdfs:isDefinedBy <https://enterprivacy.com/wp-content/uploads/2018/09/Categories-of-Personal-Information.pdf> ;
    rdfs:subClassOf dpv:Demographic ;
    sw:term_status "accepted"@en .

dpv:IncreaseServiceRobustness a rdfs:Class ;
    rdfs:label "Increase Service Robustness"@en ;
    dct:created "2018-12-10"^^xsd:date ;
    dct:creator "Axel Polleres"^^xsd:string,
        "Elmar Kiesling"^^xsd:string,
        "Fajar Ekaputra"^^xsd:string,
        "Harshvardhan J. Pandit"^^xsd:string,
        "Javier Fernandez"^^xsd:string,
        "Simon Steyskal"^^xsd:string ;
    dct:date-accepted "2019-04-05"^^xsd:date ;
    dct:description "To improve the robustness and resilience of services"@en ;
    rdfs:isDefinedBy <https://www.w3.org/community/dpvcg/wiki/Purposes_for_handling_Personal_Data#High-level_categories_.28to-be-discussed.29> ;
    rdfs:subClassOf dpv:OptimisationForController ;
    sw:term_status "accepted"@en .

dpv:IndividualHealthHistory a rdfs:Class ;
    rdfs:label "Individual Health History"@en ;
    dct:created "2019-04-04"^^xsd:date ;
    dct:creator "Elmar Kiesling; Harshvardhan J. Pandit"^^xsd:string,
        "Fajar Ekaputra"^^xsd:string ;
    dct:date-accepted "2019-06-04"^^xsd:date ;
    dct:description "Information related to an individual's information health history."@en ;
    rdfs:isDefinedBy <https://enterprivacy.com/wp-content/uploads/2018/09/Categories-of-Personal-Information.pdf> ;
    rdfs:subClassOf dpv:HealthHistory ;
    sw:term_status "accepted"@en .

dpv:Intention a rdfs:Class ;
    rdfs:label "Intention"@en ;
    dct:created "2019-04-04"^^xsd:date ;
    dct:creator "Elmar Kiesling; Harshvardhan J. Pandit"^^xsd:string,
        "Fajar Ekaputra"^^xsd:string ;
    dct:date-accepted "2019-06-04"^^xsd:date ;
    dct:description "Information about an individual's intentions"@en ;
    rdfs:isDefinedBy <https://enterprivacy.com/wp-content/uploads/2018/09/Categories-of-Personal-Information.pdf> ;
    rdfs:subClassOf dpv:Preference ;
    sw:term_status "accepted"@en .

dpv:Interaction a rdfs:Class ;
    rdfs:label "Interaction"@en ;
    dct:created "2019-04-04"^^xsd:date ;
    dct:creator "Elmar Kiesling; Harshvardhan J. Pandit"^^xsd:string,
        "Fajar Ekaputra"^^xsd:string ;
    dct:date-accepted "2019-06-04"^^xsd:date ;
    dct:description "Information about an individual's interactions in the public sphere"@en ;
    rdfs:isDefinedBy <https://enterprivacy.com/wp-content/uploads/2018/09/Categories-of-Personal-Information.pdf> ;
    rdfs:subClassOf dpv:PublicLife ;
    sw:term_status "accepted"@en .

dpv:Interest a rdfs:Class ;
    rdfs:label "Interest"@en ;
    dct:created "2019-04-04"^^xsd:date ;
    dct:creator "Elmar Kiesling; Harshvardhan J. Pandit"^^xsd:string,
        "Fajar Ekaputra"^^xsd:string ;
    dct:date-accepted "2019-06-04"^^xsd:date ;
    dct:description "Information about an individual's interests"@en ;
    rdfs:isDefinedBy <https://enterprivacy.com/wp-content/uploads/2018/09/Categories-of-Personal-Information.pdf> ;
    rdfs:subClassOf dpv:Preference ;
    sw:term_status "accepted"@en .

dpv:Internal a rdfs:Class ;
    rdfs:label "Internal"@en ;
    dct:created "2019-04-04"^^xsd:date ;
    dct:creator "Elmar Kiesling; Harshvardhan J. Pandit"^^xsd:string,
        "Fajar Ekaputra"^^xsd:string ;
    dct:date-accepted "2019-06-04"^^xsd:date ;
    dct:description "Personal data about characteristics of an individual that are internal i.e. cannot be seen or observed"@en ;
    rdfs:isDefinedBy <https://enterprivacy.com/wp-content/uploads/2018/09/Categories-of-Personal-Information.pdf> ;
    rdfs:subClassOf dpv:PersonalDataCategory ;
    sw:term_status "accepted"@en .

dpv:InternalResourceOptimisation a rdfs:Class ;
    rdfs:label "Internal Resource Optimisation"@en ;
    dct:created "2018-12-10"^^xsd:date ;
    dct:creator "Axel Polleres"^^xsd:string,
        "Elmar Kiesling"^^xsd:string,
        "Fajar Ekaputra"^^xsd:string,
        "Harshvardhan J. Pandit"^^xsd:string,
        "Javier Fernandez"^^xsd:string,
        "Simon Steyskal"^^xsd:string ;
    dct:date-accepted "2019-04-05"^^xsd:date ;
    dct:description "Optimisation of internal resources used by the organisation e.g. resource usage"@en ;
    rdfs:isDefinedBy <https://www.w3.org/community/dpvcg/wiki/Purposes_for_handling_Personal_Data#High-level_categories_.28to-be-discussed.29> ;
    rdfs:subClassOf dpv:OptimisationForController ;
    sw:term_status "accepted"@en .

dpv:Job a rdfs:Class ;
    rdfs:label "Job"@en ;
    dct:created "2019-04-04"^^xsd:date ;
    dct:creator "Elmar Kiesling; Harshvardhan J. Pandit"^^xsd:string,
        "Fajar Ekaputra"^^xsd:string ;
    dct:date-accepted "2019-06-04"^^xsd:date ;
    dct:description "Information about an individual's professional jobs"@en ;
    rdfs:isDefinedBy <https://enterprivacy.com/wp-content/uploads/2018/09/Categories-of-Personal-Information.pdf> ;
    rdfs:subClassOf dpv:Professional ;
    sw:term_status "accepted"@en .

dpv:KnowledgeBelief a rdfs:Class ;
    rdfs:label "Knowledge and Beliefs"@en ;
    dct:created "2019-04-04"^^xsd:date ;
    dct:creator "Elmar Kiesling; Harshvardhan J. Pandit"^^xsd:string,
        "Fajar Ekaputra"^^xsd:string ;
    dct:date-accepted "2019-06-04"^^xsd:date ;
    dct:description "Information about what a person knows or believes"@en ;
    rdfs:isDefinedBy <https://enterprivacy.com/wp-content/uploads/2018/09/Categories-of-Personal-Information.pdf> ;
    rdfs:subClassOf dpv:Internal ;
    sw:term_status "accepted"@en .

dpv:Language a rdfs:Class ;
    rdfs:label "Language"@en ;
    dct:created "2019-04-04"^^xsd:date ;
    dct:creator "Elmar Kiesling; Harshvardhan J. Pandit"^^xsd:string,
        "Fajar Ekaputra"^^xsd:string ;
    dct:date-accepted "2019-06-04"^^xsd:date ;
    dct:description "Information related to an individual's language."@en ;
    rdfs:isDefinedBy <https://enterprivacy.com/wp-content/uploads/2018/09/Categories-of-Personal-Information.pdf> ;
    rdfs:subClassOf dpv:Ethnicity ;
    sw:term_status "accepted"@en .

dpv:LegalAgreement a rdfs:Class ;
    rdfs:label "Legal Agreement"@en ;
    dct:created "2019-04-04"^^xsd:date ;
    dct:creator "Axel Polleres"^^xsd:string,
        "Harshvardhan J. Pandit"^^xsd:string,
        "Mark Lizar"^^xsd:string,
        "Rob Brennan"^^xsd:string ;
    dct:date-accepted "2019-04-05"^^xsd:date ;
    dct:description "A legally binding agreement"@en ;
    rdfs:isDefinedBy "DPVCG"^^xsd:string ;
    rdfs:subClassOf dpv:OrganisationalMeasure ;
    sw:term_status "accepted"@en .

dpv:LegalBasis a rdfs:Class ;
    rdfs:label "Legal Basis"@en ;
    dct:created "2019-04-04"^^xsd:date ;
    dct:date-accepted "2019-04-05"^^xsd:date ;
    dct:description "A particular legal Basis, which permits personal Data handling (e.g. Consent, etc.)"@en ;
    rdfs:isDefinedBy "DPVCG"^^xsd:string ;
    sw:term_status "accepted"@en .

dpv:LegalEntity a rdfs:Class ;
    rdfs:label "Legal Entity"@en ;
    dct:created "2019-04-04"^^xsd:date ;
    dct:date-accepted "2019-04-05"^^xsd:date ;
    dct:description "A Person or Organisation, including Data Subjects, that constitute as a legal entity."@en ;
    rdfs:subClassOf prov:Agent ;
    sw:term_status "accepted"@en .

dpv:LifeHistory a rdfs:Class ;
    rdfs:label "Life History"@en ;
    dct:created "2019-04-04"^^xsd:date ;
    dct:creator "Elmar Kiesling; Harshvardhan J. Pandit"^^xsd:string,
        "Fajar Ekaputra"^^xsd:string ;
    dct:date-accepted "2019-06-04"^^xsd:date ;
    dct:description "Information about an individual’s personal history (e.g., events that happened in a person’s life, either to them or just around them which might have influenced them (WWII, 9/11))."@en ;
    rdfs:isDefinedBy <https://enterprivacy.com/wp-content/uploads/2018/09/Categories-of-Personal-Information.pdf> ;
    rdfs:subClassOf dpv:Historical ;
    sw:term_status "accepted"@en .

dpv:Like a rdfs:Class ;
    rdfs:label "Like"@en ;
    dct:created "2019-04-04"^^xsd:date ;
    dct:creator "Elmar Kiesling; Harshvardhan J. Pandit"^^xsd:string,
        "Fajar Ekaputra"^^xsd:string ;
    dct:date-accepted "2019-06-04"^^xsd:date ;
    dct:description "Information relating to a user's likes."@en ;
    rdfs:isDefinedBy <https://enterprivacy.com/wp-content/uploads/2018/09/Categories-of-Personal-Information.pdf> ;
    rdfs:subClassOf dpv:Interest ;
    sw:term_status "accepted"@en .

dpv:LinkClicked a rdfs:Class ;
    rdfs:label "LinkClicked"@en ;
    dct:created "2019-04-04"^^xsd:date ;
    dct:creator "Elmar Kiesling; Harshvardhan J. Pandit"^^xsd:string,
        "Fajar Ekaputra"^^xsd:string ;
    dct:date-accepted "2019-06-04"^^xsd:date ;
    dct:description "Information on the links that an individual has clicked."@en ;
    rdfs:isDefinedBy <https://enterprivacy.com/wp-content/uploads/2018/09/Categories-of-Personal-Information.pdf> ;
    rdfs:seeAlso svd:Navigation ;
    rdfs:subClassOf dpv:Behavioral ;
    sw:term_status "accepted"@en .

dpv:LoanRecord a rdfs:Class ;
    rdfs:label "Loan Record"@en ;
    dct:created "2019-04-04"^^xsd:date ;
    dct:creator "Elmar Kiesling; Harshvardhan J. Pandit"^^xsd:string,
        "Fajar Ekaputra"^^xsd:string ;
    dct:date-accepted "2019-06-04"^^xsd:date ;
    dct:description "Information about loans provided or related to the individual"@en ;
    rdfs:isDefinedBy <https://enterprivacy.com/wp-content/uploads/2018/09/Categories-of-Personal-Information.pdf> ;
    rdfs:subClassOf dpv:Transactional ;
    sw:term_status "accepted"@en .

dpv:Location a rdfs:Class ;
    rdfs:label "Location"@en ;
    dct:created "2019-04-04"^^xsd:date ;
    dct:creator "Elmar Kiesling; Harshvardhan J. Pandit"^^xsd:string,
        "Fajar Ekaputra"^^xsd:string ;
    dct:date-accepted "2019-06-04"^^xsd:date ;
    dct:description "Information about an individual’s location"@en ;
    rdfs:isDefinedBy <https://enterprivacy.com/wp-content/uploads/2018/09/Categories-of-Personal-Information.pdf> ;
    rdfs:seeAlso svd:Location ;
    rdfs:subClassOf dpv:Tracking ;
    sw:term_status "accepted"@en .

dpv:MACAddress a rdfs:Class ;
    rdfs:label "MAC Address"@en ;
    dct:created "2019-04-04"^^xsd:date ;
    dct:creator "Elmar Kiesling; Harshvardhan J. Pandit"^^xsd:string,
        "Fajar Ekaputra"^^xsd:string ;
    dct:date-accepted "2019-06-04"^^xsd:date ;
    dct:description "A Media Access Control (MAC) address of a device used by an individual."@en ;
    rdfs:isDefinedBy <https://enterprivacy.com/wp-content/uploads/2018/09/Categories-of-Personal-Information.pdf> ;
    rdfs:subClassOf dpv:DeviceBased ;
    sw:term_status "accepted"@en .

dpv:MakeAvailable a rdfs:Class ;
    rdfs:label "Make Available"@en ;
    dct:created "2019-04-04"^^xsd:date ;
    dct:date-accepted "2019-05-07"^^xsd:date ;
    dct:description "to transform or publish data to be used"@en ;
    rdfs:isDefinedBy <https://eur-lex.europa.eu/eli/reg/2016/679/art_4/par_2/oj> ;
    rdfs:subClassOf dpv:Disclose ;
    sw:term_status "accepted"@en .

dpv:MaritalStatus a rdfs:Class ;
    rdfs:label "Marital Status"@en ;
    dct:created "2019-04-04"^^xsd:date ;
    dct:creator "Elmar Kiesling; Harshvardhan J. Pandit"^^xsd:string,
        "Fajar Ekaputra"^^xsd:string ;
    dct:date-accepted "2019-06-04"^^xsd:date ;
    dct:description "Information about an individual's marital status and history"@en ;
    rdfs:isDefinedBy <https://enterprivacy.com/wp-content/uploads/2018/09/Categories-of-Personal-Information.pdf> ;
    rdfs:subClassOf dpv:PublicLife ;
    sw:term_status "accepted"@en .

dpv:Marriage a rdfs:Class ;
    rdfs:label "Marriage"@en ;
    dct:created "2019-04-04"^^xsd:date ;
    dct:creator "Elmar Kiesling; Harshvardhan J. Pandit"^^xsd:string,
        "Fajar Ekaputra"^^xsd:string ;
    dct:date-accepted "2019-06-04"^^xsd:date ;
    dct:description "Information about an individual's marriage(s)."@en ;
    rdfs:isDefinedBy <https://enterprivacy.com/wp-content/uploads/2018/09/Categories-of-Personal-Information.pdf> ;
    rdfs:subClassOf dpv:FamilyStructure ;
    sw:term_status "accepted"@en .

dpv:MedicalHealth a rdfs:Class ;
    rdfs:label "MedicalHealth"@en ;
    dct:created "2019-04-04"^^xsd:date ;
    dct:creator "Elmar Kiesling; Harshvardhan J. Pandit"^^xsd:string,
        "Fajar Ekaputra"^^xsd:string ;
    dct:date-accepted "2019-06-04"^^xsd:date ;
    dct:description "Information that describes an individual’s health, medical conditions or health care"@en ;
    rdfs:isDefinedBy <https://enterprivacy.com/wp-content/uploads/2018/09/Categories-of-Personal-Information.pdf> ;
    rdfs:subClassOf dpv:External,
        dpv:SpecialCategoryPersonalData ;
    sw:term_status "accepted"@en .

dpv:MentalHealth a rdfs:Class ;
    rdfs:label "Mental Health"@en ;
    dct:created "2019-04-04"^^xsd:date ;
    dct:creator "Elmar Kiesling; Harshvardhan J. Pandit"^^xsd:string,
        "Fajar Ekaputra"^^xsd:string ;
    dct:date-accepted "2019-06-04"^^xsd:date ;
    dct:description "Information related to an individual's mental health."@en ;
    rdfs:isDefinedBy <https://enterprivacy.com/wp-content/uploads/2018/09/Categories-of-Personal-Information.pdf> ;
    rdfs:subClassOf dpv:Health ;
    sw:term_status "accepted"@en .

dpv:Move a rdfs:Class ;
    rdfs:label "Move"@en ;
    dct:created "2019-04-04"^^xsd:date ;
    dct:date-accepted "2019-05-07"^^xsd:date ;
    dct:description "to move data from one location to another including deleting the original copy"@en ;
    rdfs:isDefinedBy <https://www.specialprivacy.eu/vocabs/processing> ;
    rdfs:seeAlso svpr:Move ;
    rdfs:subClassOf dpv:Transfer ;
    sw:term_status "accepted"@en .

dpv:NDA a rdfs:Class ;
    rdfs:label "NDA"@en ;
    dct:created "2019-04-04"^^xsd:date ;
    dct:creator "Axel Polleres"^^xsd:string,
        "Harshvardhan J. Pandit"^^xsd:string,
        "Mark Lizar"^^xsd:string,
        "Rob Brennan"^^xsd:string ;
    dct:date-accepted "2019-04-05"^^xsd:date ;
    dct:description "Non-disclosure Agreements e.g. preserving confidentiality of information"@en ;
    rdfs:isDefinedBy "DPVCG"^^xsd:string ;
    rdfs:subClassOf dpv:LegalAgreement ;
    sw:term_status "accepted"@en .

dpv:Name a rdfs:Class ;
    rdfs:label "Name"@en ;
    dct:created "2019-04-04"^^xsd:date ;
    dct:creator "Elmar Kiesling; Harshvardhan J. Pandit"^^xsd:string,
        "Fajar Ekaputra"^^xsd:string ;
    dct:date-accepted "2019-06-04"^^xsd:date ;
    dct:description "A name associated with an individual e.g. given name, nickname."@en ;
    rdfs:isDefinedBy <https://enterprivacy.com/wp-content/uploads/2018/09/Categories-of-Personal-Information.pdf> ;
    rdfs:subClassOf dpv:Identifying ;
    sw:term_status "accepted"@en .

dpv:NonCommercialResearch a rdfs:Class ;
    rdfs:label "Non-Commercial Research"@en ;
    dct:created "2018-12-10"^^xsd:date ;
    dct:creator "Axel Polleres"^^xsd:string,
        "Elmar Kiesling"^^xsd:string,
        "Fajar Ekaputra"^^xsd:string,
        "Harshvardhan J. Pandit"^^xsd:string,
        "Javier Fernandez"^^xsd:string,
        "Simon Steyskal"^^xsd:string ;
    dct:date-accepted "2019-04-05"^^xsd:date ;
    dct:description "Research conducted in a non-commercial setting e.g. for a non-profit-organisation (NGO)"@en ;
    rdfs:isDefinedBy <https://www.w3.org/community/dpvcg/wiki/Purposes_for_handling_Personal_Data#High-level_categories_.28to-be-discussed.29> ;
    rdfs:subClassOf dpv:ResearchAndDevelopment ;
    sw:term_status "accepted"@en .

dpv:Obtain a rdfs:Class ;
    rdfs:label "Obtain"@en ;
    dct:created "2019-04-04"^^xsd:date ;
    dct:date-accepted "2019-05-07"^^xsd:date ;
    dct:description "to solicit or gather data from someone"@en ;
    rdfs:isDefinedBy "DPVCG"^^xsd:string ;
    rdfs:subClassOf dpv:Processing ;
    sw:term_status "accepted"@en .

dpv:OfficialID a rdfs:Class ;
    rdfs:label "Official ID"@en ;
    dct:created "2019-04-04"^^xsd:date ;
    dct:creator "Elmar Kiesling; Harshvardhan J. Pandit"^^xsd:string,
        "Fajar Ekaputra"^^xsd:string ;
    dct:date-accepted "2019-06-04"^^xsd:date ;
    dct:description "Information on an official identification document used by an individual."@en ;
    rdfs:isDefinedBy <https://enterprivacy.com/wp-content/uploads/2018/09/Categories-of-Personal-Information.pdf> ;
    rdfs:seeAlso svd:Government ;
    rdfs:subClassOf dpv:Identifying ;
    sw:term_status "accepted"@en .

dpv:Offspring a rdfs:Class ;
    rdfs:label "Offspring"@en ;
    dct:created "2019-04-04"^^xsd:date ;
    dct:creator "Elmar Kiesling; Harshvardhan J. Pandit"^^xsd:string,
        "Fajar Ekaputra"^^xsd:string ;
    dct:date-accepted "2019-06-04"^^xsd:date ;
    dct:description "Information about an individual's offspring(s)."@en ;
    rdfs:isDefinedBy <https://enterprivacy.com/wp-content/uploads/2018/09/Categories-of-Personal-Information.pdf> ;
    rdfs:subClassOf dpv:FamilyStructure ;
    sw:term_status "accepted"@en .

dpv:Opinion a rdfs:Class ;
    rdfs:label "Opinion"@en ;
    dct:created "2019-04-04"^^xsd:date ;
    dct:creator "Elmar Kiesling; Harshvardhan J. Pandit"^^xsd:string,
        "Fajar Ekaputra"^^xsd:string ;
    dct:date-accepted "2019-06-04"^^xsd:date ;
    dct:description "Information about an individual's opinions"@en ;
    rdfs:isDefinedBy <https://enterprivacy.com/wp-content/uploads/2018/09/Categories-of-Personal-Information.pdf> ;
    rdfs:subClassOf dpv:Preference ;
    sw:term_status "accepted"@en .

dpv:OptimisationForConsumer a rdfs:Class ;
    rdfs:label "Optimisation for Consumer"@en ;
    dct:created "2018-12-10"^^xsd:date ;
    dct:creator "Axel Polleres"^^xsd:string,
        "Elmar Kiesling"^^xsd:string,
        "Fajar Ekaputra"^^xsd:string,
        "Harshvardhan J. Pandit"^^xsd:string,
        "Javier Fernandez"^^xsd:string,
        "Simon Steyskal"^^xsd:string ;
    dct:date-accepted "2019-04-05"^^xsd:date ;
    dct:description "Optimisation of activities and services for the consumer or user"@en ;
    rdfs:isDefinedBy <https://www.w3.org/community/dpvcg/wiki/Purposes_for_handling_Personal_Data#High-level_categories_.28to-be-discussed.29> ;
    rdfs:seeAlso svpu:Custom ;
    rdfs:subClassOf dpv:ServiceOptimization ;
    sw:term_status "accepted"@en .

dpv:OptimisationForController a rdfs:Class ;
    rdfs:label "Optimisation for Controller"@en ;
    dct:created "2018-12-10"^^xsd:date ;
    dct:creator "Axel Polleres"^^xsd:string,
        "Elmar Kiesling"^^xsd:string,
        "Fajar Ekaputra"^^xsd:string,
        "Harshvardhan J. Pandit"^^xsd:string,
        "Javier Fernandez"^^xsd:string,
        "Simon Steyskal"^^xsd:string ;
    dct:date-accepted "2019-04-05"^^xsd:date ;
    dct:description "Optimisation of activities and services for the Controller"@en ;
    rdfs:isDefinedBy <https://www.w3.org/community/dpvcg/wiki/Purposes_for_handling_Personal_Data#High-level_categories_.28to-be-discussed.29> ;
    rdfs:subClassOf dpv:ServiceOptimization ;
    sw:term_status "accepted"@en .

dpv:OptimiseUserInterface a rdfs:Class ;
    rdfs:label "Optimise User Interface"@en ;
    dct:created "2018-12-10"^^xsd:date ;
    dct:creator "Axel Polleres"^^xsd:string,
        "Elmar Kiesling"^^xsd:string,
        "Fajar Ekaputra"^^xsd:string,
        "Harshvardhan J. Pandit"^^xsd:string,
        "Javier Fernandez"^^xsd:string,
        "Simon Steyskal"^^xsd:string ;
    dct:date-accepted "2019-04-05"^^xsd:date ;
    dct:description "Optimisation of interfaces presented to the user"@en ;
    rdfs:isDefinedBy <https://www.w3.org/community/dpvcg/wiki/Purposes_for_handling_Personal_Data#High-level_categories_.28to-be-discussed.29> ;
    rdfs:subClassOf dpv:OptimisationForConsumer ;
    sw:term_status "accepted"@en .

dpv:OrganisationalMeasure a rdfs:Class ;
    rdfs:label "Organisational Measure"@en ;
    dct:created "2019-04-04"^^xsd:date ;
    dct:creator "Axel Polleres"^^xsd:string,
        "Harshvardhan J. Pandit"^^xsd:string,
        "Mark Lizar"^^xsd:string,
        "Rob Brennan"^^xsd:string ;
    dct:date-accepted "2019-04-05"^^xsd:date ;
    dct:description "Organisational measures required/followed when processing data of the declared category"@en ;
    rdfs:isDefinedBy "DPVCG"^^xsd:string ;
    rdfs:subClassOf dpv:TechnicalOrganisationalMeasure ;
    sw:term_status "accepted"@en .

dpv:Organise a rdfs:Class ;
    rdfs:label "Organise"@en ;
    dct:created "2019-04-04"^^xsd:date ;
    dct:date-accepted "2019-05-07"^^xsd:date ;
    dct:description "to organize data for arranging or classifying"@en ;
    rdfs:isDefinedBy <https://eur-lex.europa.eu/eli/reg/2016/679/art_4/par_2/oj> ;
    rdfs:subClassOf dpv:Organise ;
    sw:term_status "accepted"@en .

dpv:Ownership a rdfs:Class ;
    rdfs:label "Ownership"@en ;
    dct:created "2019-04-04"^^xsd:date ;
    dct:creator "Elmar Kiesling; Harshvardhan J. Pandit"^^xsd:string,
        "Fajar Ekaputra"^^xsd:string ;
    dct:date-accepted "2019-06-04"^^xsd:date ;
    dct:description "Information about things an individual has owned, rented, borrowed, possessed"@en ;
    rdfs:isDefinedBy <https://enterprivacy.com/wp-content/uploads/2018/09/Categories-of-Personal-Information.pdf> ;
    rdfs:subClassOf dpv:Financial ;
    sw:term_status "accepted"@en .

dpv:PINCode a rdfs:Class ;
    rdfs:label "PIN Code"@en ;
    dct:created "2019-04-04"^^xsd:date ;
    dct:creator "Elmar Kiesling; Harshvardhan J. Pandit"^^xsd:string,
        "Fajar Ekaputra"^^xsd:string ;
    dct:date-accepted "2019-06-04"^^xsd:date ;
    dct:description "An individual's Personal identification number (PIN) used in the process of authenticating the individual as a user accessing a system."@en ;
    rdfs:isDefinedBy <https://enterprivacy.com/wp-content/uploads/2018/09/Categories-of-Personal-Information.pdf> ;
    rdfs:subClassOf dpv:Authenticating ;
    sw:term_status "accepted"@en .

dpv:Parent a rdfs:Class ;
    rdfs:label "Parent"@en ;
    dct:created "2019-04-04"^^xsd:date ;
    dct:creator "Elmar Kiesling; Harshvardhan J. Pandit"^^xsd:string,
        "Fajar Ekaputra"^^xsd:string ;
    dct:date-accepted "2019-06-04"^^xsd:date ;
    dct:description "Information about an individual's parent(s)."@en ;
    rdfs:isDefinedBy <https://enterprivacy.com/wp-content/uploads/2018/09/Categories-of-Personal-Information.pdf> ;
    rdfs:subClassOf dpv:FamilyStructure ;
    sw:term_status "accepted"@en .

dpv:Password a rdfs:Class ;
    rdfs:label "Password"@en ;
    dct:created "2019-04-04"^^xsd:date ;
    dct:creator "Elmar Kiesling; Harshvardhan J. Pandit"^^xsd:string,
        "Fajar Ekaputra"^^xsd:string ;
    dct:date-accepted "2019-06-04"^^xsd:date ;
    dct:description "An individual's password used in the process of authenticating the individual as a user accessing a system."@en ;
    rdfs:isDefinedBy <https://enterprivacy.com/wp-content/uploads/2018/09/Categories-of-Personal-Information.pdf> ;
    rdfs:subClassOf dpv:Authenticating ;
    sw:term_status "accepted"@en .

dpv:PersonalDataCategory a rdfs:Class ;
    rdfs:label "Personal Data Category"@en ;
    dct:created "2019-04-04"^^xsd:date ;
    dct:creator "Axel Polleres"^^xsd:string,
        "Harshvardhan Pandit"^^xsd:string ;
    dct:date-accepted "2019-04-05"^^xsd:date ;
    dct:description "A category of personal data (as defined by GDPR article 4.1) from the personal data categories taxonomy, i.e. for instance denoting the category of an object/field or data item that is used for processing"@en ;
    rdfs:isDefinedBy <https://eur-lex.europa.eu/eli/reg/2016/679/art_4/par_1/pnt_g/oj>,
        "DPVCG"^^xsd:string,
        "SPECIAL"^^xsd:string ;
    rdfs:seeAlso spl:AnyData ;
    sw:term_status "accepted"@en .

dpv:PersonalDataHandling a rdfs:Class ;
    rdfs:label "Personal Data Handling"@en ;
    dct:created "2019-04-04"^^xsd:date ;
    dct:creator "Axel Polleres"^^xsd:string,
        "Javier Ferenandez"^^xsd:string ;
    dct:date-accepted "2019-04-05"^^xsd:date ;
    dct:description """Top Class to describe a concrete instance of legal personal Data Handling of a defined class of Data Subjects, meaning that a personal Data Category is undergoing specified processing by a specific data controller and/or
transferred to some recipient for a particular purpose, based on a specific legal ground, with specified security measures and restrictions (e.g. storage locations and storage durations)."""@en ;
    sw:term_status "accepted"@en .

dpv:PersonalPossession a rdfs:Class ;
    rdfs:label "Personal Possession"@en ;
    dct:created "2019-04-04"^^xsd:date ;
    dct:creator "Elmar Kiesling; Harshvardhan J. Pandit"^^xsd:string,
        "Fajar Ekaputra"^^xsd:string ;
    dct:date-accepted "2019-06-04"^^xsd:date ;
    dct:description "Information about an individual's personal possessions."@en ;
    rdfs:isDefinedBy <https://enterprivacy.com/wp-content/uploads/2018/09/Categories-of-Personal-Information.pdf> ;
    rdfs:subClassOf dpv:Ownership ;
    sw:term_status "accepted"@en .

dpv:PersonalisedBenefits a rdfs:Class ;
    rdfs:label "Personalised Benefits"@en ;
    dct:created "2018-12-10"^^xsd:date ;
    dct:creator "Axel Polleres"^^xsd:string,
        "Elmar Kiesling"^^xsd:string,
        "Fajar Ekaputra"^^xsd:string,
        "Harshvardhan J. Pandit"^^xsd:string,
        "Javier Fernandez"^^xsd:string,
        "Simon Steyskal"^^xsd:string ;
    dct:date-accepted "2019-04-05"^^xsd:date ;
    dct:description "Personalisation of benefits received by the user"@en ;
    rdfs:isDefinedBy <https://www.w3.org/community/dpvcg/wiki/Purposes_for_handling_Personal_Data#High-level_categories_.28to-be-discussed.29> ;
    rdfs:subClassOf dpv:ServicePersonalization ;
    sw:term_status "accepted"@en .

dpv:Personality a rdfs:Class ;
    rdfs:label "Personality"@en ;
    dct:created "2019-04-04"^^xsd:date ;
    dct:creator "Elmar Kiesling; Harshvardhan J. Pandit"^^xsd:string,
        "Fajar Ekaputra"^^xsd:string ;
    dct:date-accepted "2019-06-04"^^xsd:date ;
    dct:description "Information that relates to an individual's personality (e.g., categorization in terms of the Big Five personality traits)"@en ;
    rdfs:isDefinedBy <https://enterprivacy.com/wp-content/uploads/2018/09/Categories-of-Personal-Information.pdf> ;
    rdfs:subClassOf dpv:Behavioral ;
    sw:term_status "accepted"@en .

dpv:PhilosophicalBelief a rdfs:Class ;
    rdfs:label "Philosophical Belief"@en ;
    dct:created "2019-04-04"^^xsd:date ;
    dct:creator "Elmar Kiesling; Harshvardhan J. Pandit"^^xsd:string,
        "Fajar Ekaputra"^^xsd:string ;
    dct:date-accepted "2019-06-04"^^xsd:date ;
    dct:description "Information about an individual’s philosophical beliefs."@en ;
    rdfs:isDefinedBy <https://enterprivacy.com/wp-content/uploads/2018/09/Categories-of-Personal-Information.pdf> ;
    rdfs:subClassOf dpv:KnowledgeBelief,
        dpv:SpecialCategoryPersonalData ;
    sw:term_status "accepted"@en .

dpv:PhysicalAddress a rdfs:Class ;
    rdfs:label "Physical Address"@en ;
    dct:created "2019-04-04"^^xsd:date ;
    dct:creator "Elmar Kiesling; Harshvardhan J. Pandit"^^xsd:string,
        "Fajar Ekaputra"^^xsd:string ;
    dct:date-accepted "2019-06-04"^^xsd:date ;
    dct:description "Information about an individual's physical address."@en ;
    rdfs:isDefinedBy <https://enterprivacy.com/wp-content/uploads/2018/09/Categories-of-Personal-Information.pdf> ;
    rdfs:subClassOf dpv:Contact ;
    sw:term_status "accepted"@en .

dpv:PhysicalCharacteristic a rdfs:Class ;
    rdfs:label "PhysicalCharacteristic"@en ;
    dct:created "2019-04-04"^^xsd:date ;
    dct:creator "Elmar Kiesling; Harshvardhan J. Pandit"^^xsd:string,
        "Fajar Ekaputra"^^xsd:string ;
    dct:date-accepted "2019-06-04"^^xsd:date ;
    dct:description "Information that describes an individual’s physical characteristics"@en ;
    rdfs:isDefinedBy <https://enterprivacy.com/wp-content/uploads/2018/09/Categories-of-Personal-Information.pdf> ;
    rdfs:seeAlso svd:Demographic ;
    rdfs:subClassOf dpv:External ;
    sw:term_status "accepted"@en .

dpv:PhysicalHealth a rdfs:Class ;
    rdfs:label "Physical Health"@en ;
    dct:created "2019-04-04"^^xsd:date ;
    dct:creator "Elmar Kiesling; Harshvardhan J. Pandit"^^xsd:string,
        "Fajar Ekaputra"^^xsd:string ;
    dct:date-accepted "2019-06-04"^^xsd:date ;
    dct:description "Information related to an individual's physical health."@en ;
    rdfs:isDefinedBy <https://enterprivacy.com/wp-content/uploads/2018/09/Categories-of-Personal-Information.pdf> ;
    rdfs:subClassOf dpv:Health ;
    sw:term_status "accepted"@en .

dpv:PhysicalTrait a rdfs:Class ;
    rdfs:label "Physical Trait"@en ;
    dct:created "2019-04-04"^^xsd:date ;
    dct:creator "Elmar Kiesling; Harshvardhan J. Pandit"^^xsd:string,
        "Fajar Ekaputra"^^xsd:string ;
    dct:date-accepted "2019-06-04"^^xsd:date ;
    dct:description "Information on defining traits or features about an individuals body."@en ;
    rdfs:isDefinedBy <https://enterprivacy.com/wp-content/uploads/2018/09/Categories-of-Personal-Information.pdf> ;
    rdfs:subClassOf dpv:Demographic ;
    sw:term_status "accepted"@en .

dpv:Picture a rdfs:Class ;
    rdfs:label "Picture"@en ;
    dct:created "2019-04-04"^^xsd:date ;
    dct:creator "Elmar Kiesling; Harshvardhan J. Pandit"^^xsd:string,
        "Fajar Ekaputra"^^xsd:string ;
    dct:date-accepted "2019-06-04"^^xsd:date ;
    dct:description "A visual representation or image of an individual e.g. profile photo."@en ;
    rdfs:isDefinedBy <https://enterprivacy.com/wp-content/uploads/2018/09/Categories-of-Personal-Information.pdf> ;
    rdfs:subClassOf dpv:Identifying ;
    sw:term_status "accepted"@en .

dpv:Piercing a rdfs:Class ;
    rdfs:label "Piercing"@en ;
    dct:created "2019-04-04"^^xsd:date ;
    dct:creator "Elmar Kiesling; Harshvardhan J. Pandit"^^xsd:string,
        "Fajar Ekaputra"^^xsd:string ;
    dct:date-accepted "2019-06-04"^^xsd:date ;
    dct:description "Information about an individual's piercings"@en ;
    rdfs:isDefinedBy <https://enterprivacy.com/wp-content/uploads/2018/09/Categories-of-Personal-Information.pdf> ;
    rdfs:subClassOf dpv:PhysicalCharacteristic ;
    sw:term_status "accepted"@en .

dpv:PoliticalAffiliation a rdfs:Class ;
    rdfs:label "Political Affiliation"@en ;
    dct:created "2019-04-04"^^xsd:date ;
    dct:creator "Elmar Kiesling; Harshvardhan J. Pandit"^^xsd:string,
        "Fajar Ekaputra"^^xsd:string ;
    dct:date-accepted "2019-06-04"^^xsd:date ;
    dct:description "Information about an individual's political affiliation and history"@en ;
    rdfs:isDefinedBy <https://enterprivacy.com/wp-content/uploads/2018/09/Categories-of-Personal-Information.pdf> ;
    rdfs:seeAlso svd:Political ;
    rdfs:subClassOf dpv:PublicLife,
        dpv:SpecialCategoryPersonalData ;
    sw:term_status "accepted"@en .

dpv:Preference a rdfs:Class ;
    rdfs:label "Preference"@en ;
    dct:created "2019-04-04"^^xsd:date ;
    dct:creator "Elmar Kiesling; Harshvardhan J. Pandit"^^xsd:string,
        "Fajar Ekaputra"^^xsd:string ;
    dct:date-accepted "2019-06-04"^^xsd:date ;
    dct:description "Information about an individual’s preferences or interests"@en ;
    rdfs:isDefinedBy <https://enterprivacy.com/wp-content/uploads/2018/09/Categories-of-Personal-Information.pdf> ;
    rdfs:seeAlso svd:Preference ;
    rdfs:subClassOf dpv:Internal ;
    sw:term_status "accepted"@en .

dpv:Prescription a rdfs:Class ;
    rdfs:label "Prescription"@en ;
    dct:created "2019-04-04"^^xsd:date ;
    dct:creator "Elmar Kiesling; Harshvardhan J. Pandit"^^xsd:string,
        "Fajar Ekaputra"^^xsd:string ;
    dct:date-accepted "2019-06-04"^^xsd:date ;
    dct:description "Information about prescriptions made for an individual."@en ;
    rdfs:isDefinedBy <https://enterprivacy.com/wp-content/uploads/2018/09/Categories-of-Personal-Information.pdf> ;
    rdfs:subClassOf dpv:MedicalHealth ;
    sw:term_status "accepted"@en .

dpv:PrivacyByDefault a rdfs:Class ;
    rdfs:label "Privacy by Default"@en ;
    dct:created "2019-04-04"^^xsd:date ;
    dct:creator "Axel Polleres"^^xsd:string,
        "Harshvardhan J. Pandit"^^xsd:string,
        "Mark Lizar"^^xsd:string,
        "Rob Brennan"^^xsd:string ;
    dct:date-accepted "2019-04-05"^^xsd:date ;
    dct:description "Practices regarding selecting appropriate data protection and privacy measures as the 'default' in an activity or service"@en ;
    rdfs:isDefinedBy "DPVCG"^^xsd:string ;
    rdfs:subClassOf dpv:GuidelinesPrinciple ;
    sw:term_status "accepted"@en .

dpv:PrivacyByDesign a rdfs:Class ;
    rdfs:label "Privacy by Design"@en ;
    dct:created "2019-04-04"^^xsd:date ;
    dct:creator "Axel Polleres"^^xsd:string,
        "Harshvardhan J. Pandit"^^xsd:string,
        "Mark Lizar"^^xsd:string,
        "Rob Brennan"^^xsd:string ;
    dct:date-accepted "2019-04-05"^^xsd:date ;
    dct:description "Practices regarding incorporating data protection and privacy in the design of information and services"@en ;
    rdfs:isDefinedBy "DPVCG"^^xsd:string ;
    rdfs:subClassOf dpv:RiskManagementProcedure ;
    sw:term_status "accepted"@en .

dpv:PrivacyPreference a rdfs:Class ;
    rdfs:label "Privacy Preference"@en ;
    dct:created "2019-04-04"^^xsd:date ;
    dct:creator "Elmar Kiesling; Harshvardhan J. Pandit"^^xsd:string,
        "Fajar Ekaputra"^^xsd:string ;
    dct:date-accepted "2019-06-04"^^xsd:date ;
    dct:description "Information about an individual's privacy preferences"@en ;
    rdfs:isDefinedBy <https://enterprivacy.com/wp-content/uploads/2018/09/Categories-of-Personal-Information.pdf> ;
    rdfs:subClassOf dpv:Preference ;
    sw:term_status "accepted"@en .

dpv:Processing a rdfs:Class ;
    rdfs:label "Processing"@en ;
    dct:created "2019-04-04"^^xsd:date ;
    dct:creator "Axel Polleres"^^xsd:string,
        "Javier Ferenandez"^^xsd:string ;
    dct:date-accepted "2019-04-05"^^xsd:date ;
    dct:description "A type of processing from one of the processing categories in the processing Taxonomy"@en ;
    rdfs:isDefinedBy "DPVCG"^^xsd:string,
        "SPECIAL"^^xsd:string ;
    rdfs:seeAlso spl:AnyProcessing ;
    rdfs:subClassOf odrl:Action ;
    sw:term_status "accepted"@en .

dpv:Proclivitie a rdfs:Class ;
    rdfs:label "Proclivitie"@en ;
    dct:created "2019-04-04"^^xsd:date ;
    dct:creator "Elmar Kiesling; Harshvardhan J. Pandit"^^xsd:string,
        "Fajar Ekaputra"^^xsd:string ;
    dct:date-accepted "2019-06-04"^^xsd:date ;
    dct:description "Information about an individual's proclivities in a sexual context"@en ;
    rdfs:isDefinedBy <https://enterprivacy.com/wp-content/uploads/2018/09/Categories-of-Personal-Information.pdf> ;
    rdfs:subClassOf dpv:Sexual ;
    sw:term_status "accepted"@en .

dpv:Professional a rdfs:Class ;
    rdfs:label "Professional"@en ;
    dct:created "2019-04-04"^^xsd:date ;
    dct:creator "Elmar Kiesling; Harshvardhan J. Pandit"^^xsd:string,
        "Fajar Ekaputra"^^xsd:string ;
    dct:date-accepted "2019-06-04"^^xsd:date ;
    dct:description "Information about an individual’s educational or professional career"@en ;
    rdfs:isDefinedBy <https://enterprivacy.com/wp-content/uploads/2018/09/Categories-of-Personal-Information.pdf> ;
    rdfs:subClassOf dpv:Social ;
    sw:term_status "accepted"@en .

dpv:ProfessionalEvaluation a rdfs:Class ;
    rdfs:label "Professional Evaluation"@en ;
    dct:created "2019-04-04"^^xsd:date ;
    dct:creator "Elmar Kiesling; Harshvardhan J. Pandit"^^xsd:string,
        "Fajar Ekaputra"^^xsd:string ;
    dct:date-accepted "2019-06-04"^^xsd:date ;
    dct:description "Information about professional evaluations associated with an individual"@en ;
    rdfs:isDefinedBy <https://enterprivacy.com/wp-content/uploads/2018/09/Categories-of-Personal-Information.pdf> ;
    rdfs:subClassOf dpv:Professional ;
    sw:term_status "accepted"@en .

dpv:ProfessionalInterview a rdfs:Class ;
    rdfs:label "Professional Interview"@en ;
    dct:created "2019-04-04"^^xsd:date ;
    dct:creator "Elmar Kiesling; Harshvardhan J. Pandit"^^xsd:string,
        "Fajar Ekaputra"^^xsd:string ;
    dct:date-accepted "2019-06-04"^^xsd:date ;
    dct:description "Information about professional interviews associated with an individual"@en ;
    rdfs:isDefinedBy <https://enterprivacy.com/wp-content/uploads/2018/09/Categories-of-Personal-Information.pdf> ;
    rdfs:subClassOf dpv:Professional ;
    sw:term_status "accepted"@en .

dpv:Profiling a rdfs:Class ;
    rdfs:label "Profiling"@en ;
    dct:created "2019-04-04"^^xsd:date ;
    dct:date-accepted "2019-05-07"^^xsd:date ;
    dct:description "to create a profile that describes or represents a person"@en ;
    rdfs:isDefinedBy "DPVCG"^^xsd:string ;
    rdfs:subClassOf dpv:Use ;
    sw:term_status "accepted"@en .

dpv:PseudoAnonymise a rdfs:Class ;
    rdfs:label "Pseudo-Anonymise"@en ;
    dct:created "2019-04-04"^^xsd:date ;
    dct:date-accepted "2019-05-07"^^xsd:date ;
    dct:description "to replace personal identifiable information by artificial identifiers"@en ;
    rdfs:isDefinedBy "DPVCG"^^xsd:string ;
    rdfs:subClassOf dpv:Transform ;
    sw:term_status "accepted"@en .

dpv:PseudoAnonymization a rdfs:Class ;
    rdfs:label "Pseudo-Anonymization"@en ;
    dct:created "2019-04-04"^^xsd:date ;
    dct:creator "Axel Polleres"^^xsd:string,
        "Harshvardhan J. Pandit"^^xsd:string,
        "Mark Lizar"^^xsd:string,
        "Rob Brennan"^^xsd:string ;
    dct:date-accepted "2019-04-05"^^xsd:date ;
    dct:description "PseudoAnonmyization or 'pseudonymisation’ means the processing of personal data in such a manner that the personal data can no longer be attributed to a specific data subject without the use of additional information, provided that such additional information is kept separately and is subject to technical and organisational measures to ensure that the personal data are not attributed to an identified or identifiable natural person;"@en ;
    rdfs:isDefinedBy <https://eur-lex.europa.eu/eli/reg/2016/679/art_4/par_5/pnt_g/oj> ;
    rdfs:subClassOf dpv:PseudonymisationEncryption ;
    sw:term_status "accepted"@en .

dpv:PseudonymisationEncryption a rdfs:Class ;
    rdfs:label "Pseudonymisation and Encryption"@en ;
    dct:created "2019-04-04"^^xsd:date ;
    dct:creator "Axel Polleres"^^xsd:string,
        "Harshvardhan J. Pandit"^^xsd:string,
        "Mark Lizar"^^xsd:string,
        "Rob Brennan"^^xsd:string ;
    dct:date-accepted "2019-04-05"^^xsd:date ;
    dct:description "Category of technical measures consisting of pseudoanonymization and encryption"@en ;
    rdfs:isDefinedBy "DPVCG"^^xsd:string ;
    rdfs:subClassOf dpv:TechnicalMeasure ;
    sw:term_status "accepted"@en .

dpv:PublicLife a rdfs:Class ;
    rdfs:label "Public Life"@en ;
    dct:created "2019-04-04"^^xsd:date ;
    dct:creator "Elmar Kiesling; Harshvardhan J. Pandit"^^xsd:string,
        "Fajar Ekaputra"^^xsd:string ;
    dct:date-accepted "2019-06-04"^^xsd:date ;
    dct:description "Information about an individual’s public life"@en ;
    rdfs:isDefinedBy <https://enterprivacy.com/wp-content/uploads/2018/09/Categories-of-Personal-Information.pdf> ;
    rdfs:subClassOf dpv:Social ;
    sw:term_status "accepted"@en .

dpv:Purchase a rdfs:Class ;
    rdfs:label "Purchase"@en ;
    dct:created "2019-04-04"^^xsd:date ;
    dct:creator "Elmar Kiesling; Harshvardhan J. Pandit"^^xsd:string,
        "Fajar Ekaputra"^^xsd:string ;
    dct:date-accepted "2019-06-04"^^xsd:date ;
    dct:description "Information about purchases such as items bought e.g. grocery or clothing"@en ;
    rdfs:isDefinedBy <https://enterprivacy.com/wp-content/uploads/2018/09/Categories-of-Personal-Information.pdf> ;
    rdfs:seeAlso svd:Purchase ;
    rdfs:subClassOf dpv:Transactional ;
    sw:term_status "accepted"@en .

dpv:PurchasesAndSpendingHabit a rdfs:Class ;
    rdfs:label "Purchases and Spending Habit"@en ;
    dct:created "2019-04-04"^^xsd:date ;
    dct:creator "Elmar Kiesling; Harshvardhan J. Pandit"^^xsd:string,
        "Fajar Ekaputra"^^xsd:string ;
    dct:date-accepted "2019-06-04"^^xsd:date ;
    dct:description "Information about analysis of purchases made and money spent expressed as a habit e.g. monthly shopping trends"@en ;
    rdfs:isDefinedBy <https://enterprivacy.com/wp-content/uploads/2018/09/Categories-of-Personal-Information.pdf> ;
    rdfs:subClassOf dpv:Transactional ;
    sw:term_status "accepted"@en .

dpv:Purpose a rdfs:Class ;
    rdfs:label "Purpose"@en ;
    dct:created "2019-04-04"^^xsd:date ;
    dct:creator "Axel Polleres"^^xsd:string,
        "Javier Ferenandez"^^xsd:string ;
    dct:date-accepted "2019-04-05"^^xsd:date ;
    dct:description "The purpose of Data Handling, from the purposes Taxonomy"@en ;
    rdfs:isDefinedBy "DPVCG"^^xsd:string,
        "SPECIAL"^^xsd:string ;
    rdfs:seeAlso spl:AnyPurpose ;
    sw:term_status "accepted"@en .

dpv:Race a rdfs:Class ;
    rdfs:label "Race"@en ;
    dct:created "2019-04-04"^^xsd:date ;
    dct:creator "Elmar Kiesling; Harshvardhan J. Pandit"^^xsd:string,
        "Fajar Ekaputra"^^xsd:string ;
    dct:date-accepted "2019-06-04"^^xsd:date ;
    dct:description "Information related to an individual's race."@en ;
    rdfs:isDefinedBy <https://enterprivacy.com/wp-content/uploads/2018/09/Categories-of-Personal-Information.pdf> ;
    rdfs:subClassOf dpv:Ethnicity,
        dpv:SpecialCategoryPersonalData ;
    sw:term_status "accepted"@en .

dpv:Recipient a rdfs:Class ;
    rdfs:label "Recipient"@en ;
    dct:created "2019-04-04"^^xsd:date ;
    dct:creator "Axel Polleres"^^xsd:string,
        "Javier Ferenandez"^^xsd:string ;
    dct:date-accepted "2019-04-05"^^xsd:date ;
    dct:description "The entities that can access the result of a data handling action/processing, any legal entity that is defined by article 4.9 of GDPR, which states - 'recipient' means a natural or legal person, public authority, agency or another body, to which the personal data are disclosed, whether a third party or not."@en ;
    rdfs:isDefinedBy <https://eur-lex.europa.eu/eli/reg/2016/679/art_4/par_9/pnt_g/oj>,
        "DPVCG"^^xsd:string,
        "SPECIAL"^^xsd:string ;
    rdfs:seeAlso spl:AnyRecipient ;
    sw:term_status "accepted"@en .

dpv:Record a rdfs:Class ;
    rdfs:label "Record"@en ;
    dct:created "2019-04-04"^^xsd:date ;
    dct:date-accepted "2019-05-07"^^xsd:date ;
    dct:description "to make a record (especially media)"@en ;
    rdfs:isDefinedBy <https://eur-lex.europa.eu/eli/reg/2016/679/art_4/par_2/oj> ;
    rdfs:subClassOf dpv:Obtain ;
    sw:term_status "accepted"@en .

dpv:Reference a rdfs:Class ;
    rdfs:label "Reference"@en ;
    dct:created "2019-04-04"^^xsd:date ;
    dct:creator "Elmar Kiesling; Harshvardhan J. Pandit"^^xsd:string,
        "Fajar Ekaputra"^^xsd:string ;
    dct:date-accepted "2019-06-04"^^xsd:date ;
    dct:description "Information about an individual's references in the professional context"@en ;
    rdfs:isDefinedBy <https://enterprivacy.com/wp-content/uploads/2018/09/Categories-of-Personal-Information.pdf> ;
    rdfs:subClassOf dpv:Professional ;
    sw:term_status "accepted"@en .

dpv:RegularityOfRecertification a rdfs:Class ;
    rdfs:label "Regularity of Re-certification"@en ;
    dct:created "2019-04-04"^^xsd:date ;
    dct:creator "Axel Polleres"^^xsd:string,
        "Harshvardhan J. Pandit"^^xsd:string,
        "Mark Lizar"^^xsd:string,
        "Rob Brennan"^^xsd:string ;
    dct:date-accepted "2019-04-05"^^xsd:date ;
    dct:description "Specifies policy regarding repetition or renewal of existing certification(s)"@en ;
    rdfs:isDefinedBy "DPVCG"^^xsd:string ;
    rdfs:subClassOf dpv:RiskManagementProcedure ;
    sw:term_status "accepted"@en .

dpv:Relationship a rdfs:Class ;
    rdfs:label "Relationship"@en ;
    dct:created "2019-04-04"^^xsd:date ;
    dct:creator "Elmar Kiesling; Harshvardhan J. Pandit"^^xsd:string,
        "Fajar Ekaputra"^^xsd:string ;
    dct:date-accepted "2019-06-04"^^xsd:date ;
    dct:description "Information that characterizes an individual's relationships with other individuals."@en ;
    rdfs:isDefinedBy <https://enterprivacy.com/wp-content/uploads/2018/09/Categories-of-Personal-Information.pdf> ;
    rdfs:subClassOf dpv:Family ;
    sw:term_status "accepted"@en .

dpv:Religion a rdfs:Class ;
    rdfs:label "Religion"@en ;
    dct:created "2019-04-04"^^xsd:date ;
    dct:creator "Elmar Kiesling; Harshvardhan J. Pandit"^^xsd:string,
        "Fajar Ekaputra"^^xsd:string ;
    dct:date-accepted "2019-06-04"^^xsd:date ;
    dct:description "Information about an individual's religion, religious inclinations, and religious history."@en ;
    rdfs:isDefinedBy <https://enterprivacy.com/wp-content/uploads/2018/09/Categories-of-Personal-Information.pdf> ;
    rdfs:subClassOf dpv:PublicLife,
        dpv:SpecialCategoryPersonalData ;
    sw:term_status "accepted"@en .

dpv:ReligiousBelief a rdfs:Class ;
    rdfs:label "Religious Belief"@en ;
    dct:created "2019-04-04"^^xsd:date ;
    dct:creator "Elmar Kiesling; Harshvardhan J. Pandit"^^xsd:string,
        "Fajar Ekaputra"^^xsd:string ;
    dct:date-accepted "2019-06-04"^^xsd:date ;
    dct:description "Information about an individual’s religious beliefs."@en ;
    rdfs:isDefinedBy <https://enterprivacy.com/wp-content/uploads/2018/09/Categories-of-Personal-Information.pdf> ;
    rdfs:subClassOf dpv:KnowledgeBelief,
        dpv:SpecialCategoryPersonalData ;
    sw:term_status "accepted"@en .

dpv:Remove a rdfs:Class ;
    rdfs:label "Remove"@en ;
    dct:created "2019-04-04"^^xsd:date ;
    dct:date-accepted "2019-05-07"^^xsd:date ;
    dct:description "to destruct or erase data"@en ;
    rdfs:isDefinedBy "DPVCG"^^xsd:string ;
    rdfs:subClassOf dpv:Processing ;
    sw:term_status "accepted"@en .

dpv:ResearchAndDevelopment a rdfs:Class ;
    rdfs:label "Research and Development"@en ;
    dct:created "2018-12-10"^^xsd:date ;
    dct:creator "Axel Polleres"^^xsd:string,
        "Elmar Kiesling"^^xsd:string,
        "Fajar Ekaputra"^^xsd:string,
        "Harshvardhan J. Pandit"^^xsd:string,
        "Javier Fernandez"^^xsd:string,
        "Simon Steyskal"^^xsd:string ;
    dct:date-accepted "2019-04-05"^^xsd:date ;
    dct:description "Performing research and developing new methods,products, or services"@en ;
    rdfs:isDefinedBy <https://www.w3.org/community/dpvcg/wiki/Purposes_for_handling_Personal_Data#High-level_categories_.28to-be-discussed.29> ;
    rdfs:subClassOf dpv:Purpose ;
    sw:term_status "accepted"@en .

dpv:Restrict a rdfs:Class ;
    rdfs:label "Restrict"@en ;
    dct:created "2019-04-04"^^xsd:date ;
    dct:date-accepted "2019-05-07"^^xsd:date ;
    dct:description "to apply a restriction on the processsing of specific records"@en ;
    rdfs:isDefinedBy <https://eur-lex.europa.eu/eli/reg/2016/679/art_4/par_2/oj> ;
    rdfs:subClassOf dpv:Transform ;
    sw:term_status "accepted"@en .

dpv:Retina a rdfs:Class ;
    rdfs:label "Retina"@en ;
    dct:created "2019-04-04"^^xsd:date ;
    dct:creator "Elmar Kiesling; Harshvardhan J. Pandit"^^xsd:string,
        "Fajar Ekaputra"^^xsd:string ;
    dct:date-accepted "2019-06-04"^^xsd:date ;
    dct:description "Information related to an individual's retina used for biometric purposes."@en ;
    rdfs:isDefinedBy <https://enterprivacy.com/wp-content/uploads/2018/09/Categories-of-Personal-Information.pdf> ;
    rdfs:subClassOf dpv:Biometric ;
    sw:term_status "accepted"@en .

dpv:Retrieve a rdfs:Class ;
    rdfs:label "Retrieve"@en ;
    dct:created "2019-04-04"^^xsd:date ;
    dct:date-accepted "2019-05-07"^^xsd:date ;
    dct:description "to retrieve data, often in an automated manner"@en ;
    rdfs:isDefinedBy <https://eur-lex.europa.eu/eli/reg/2016/679/art_4/par_2/oj> ;
    rdfs:subClassOf dpv:Use ;
    sw:term_status "accepted"@en .

dpv:RiskManagementProcedure a rdfs:Class ;
    rdfs:label "Risk Management Procedure"@en ;
    dct:created "2019-04-04"^^xsd:date ;
    dct:creator "Axel Polleres"^^xsd:string,
        "Harshvardhan J. Pandit"^^xsd:string,
        "Mark Lizar"^^xsd:string,
        "Rob Brennan"^^xsd:string ;
    dct:date-accepted "2019-04-05"^^xsd:date ;
    dct:description "Risk management refers to a coordinated set of activities and methods that is used to direct an organization and to control the many risks that can affect its ability to achieve objectives.  The term risk management also refers to the programme that is used to manage risk. This programme includes risk management principles, a risk management framework, and a risk management process."@en ;
    rdfs:comment "Data Protection Impact Assessments as per GDPR art 35, other Privacy Impact Assessments, threat severity assessment https://www.cnil.fr/en/privacy-impact-assessment-pia"@en ;
    rdfs:isDefinedBy "ISO 31000"^^xsd:string ;
    rdfs:subClassOf dpv:OrganisationalMeasure ;
    sw:term_status "accepted"@en .

dpv:RoomNumber a rdfs:Class ;
    rdfs:label "Room Number"@en ;
    dct:created "2019-04-04"^^xsd:date ;
    dct:creator "Elmar Kiesling; Harshvardhan J. Pandit"^^xsd:string,
        "Fajar Ekaputra"^^xsd:string ;
    dct:date-accepted "2019-06-04"^^xsd:date ;
    dct:description "Room number of a location associated with an individual."@en ;
    rdfs:isDefinedBy <https://enterprivacy.com/wp-content/uploads/2018/09/Categories-of-Personal-Information.pdf> ;
    rdfs:subClassOf dpv:Location ;
    sw:term_status "accepted"@en .

dpv:Salary a rdfs:Class ;
    rdfs:label "Salary"@en ;
    dct:created "2019-04-04"^^xsd:date ;
    dct:creator "Elmar Kiesling; Harshvardhan J. Pandit"^^xsd:string,
        "Fajar Ekaputra"^^xsd:string ;
    dct:date-accepted "2019-06-04"^^xsd:date ;
    dct:description "Information about an individual's salary"@en ;
    rdfs:isDefinedBy <https://enterprivacy.com/wp-content/uploads/2018/09/Categories-of-Personal-Information.pdf> ;
    rdfs:subClassOf dpv:Professional ;
    sw:term_status "accepted"@en .

dpv:Sale a rdfs:Class ;
    rdfs:label "Sale"@en ;
    dct:created "2019-04-04"^^xsd:date ;
    dct:creator "Elmar Kiesling; Harshvardhan J. Pandit"^^xsd:string,
        "Fajar Ekaputra"^^xsd:string ;
    dct:date-accepted "2019-06-04"^^xsd:date ;
    dct:description "Information about sales e.g. selling of goods or services"@en ;
    rdfs:isDefinedBy <https://enterprivacy.com/wp-content/uploads/2018/09/Categories-of-Personal-Information.pdf> ;
    rdfs:subClassOf dpv:Transactional ;
    sw:term_status "accepted"@en .

dpv:School a rdfs:Class ;
    rdfs:label "School"@en ;
    dct:created "2019-04-04"^^xsd:date ;
    dct:creator "Elmar Kiesling; Harshvardhan J. Pandit"^^xsd:string,
        "Fajar Ekaputra"^^xsd:string ;
    dct:date-accepted "2019-06-04"^^xsd:date ;
    dct:description "Information about an individual's school such as name of school, conduct, or grades obtained."@en ;
    rdfs:isDefinedBy <https://enterprivacy.com/wp-content/uploads/2018/09/Categories-of-Personal-Information.pdf> ;
    rdfs:subClassOf dpv:Professional ;
    sw:term_status "accepted"@en .

dpv:Seal a rdfs:Class ;
    rdfs:label "Seal"@en ;
    dct:created "2019-04-04"^^xsd:date ;
    dct:creator "Axel Polleres"^^xsd:string,
        "Harshvardhan J. Pandit"^^xsd:string,
        "Mark Lizar"^^xsd:string,
        "Rob Brennan"^^xsd:string ;
    dct:date-accepted "2019-04-05"^^xsd:date ;
    dct:description "a seal or a mark indicating proof of certification to some certification or standard"@en ;
    rdfs:isDefinedBy "DPVCG"^^xsd:string ;
    rdfs:subClassOf dpv:CertificationSeal ;
    sw:term_status "accepted"@en .

dpv:SecretText a rdfs:Class ;
    rdfs:label "Secret Text"@en ;
    dct:created "2019-04-04"^^xsd:date ;
    dct:creator "Elmar Kiesling; Harshvardhan J. Pandit"^^xsd:string,
        "Fajar Ekaputra"^^xsd:string ;
    dct:date-accepted "2019-06-04"^^xsd:date ;
    dct:description "An individual's secret text used in the process of authenticating the individual as a user accessing a system, e.g., when recovering a lost password."@en ;
    rdfs:isDefinedBy <https://enterprivacy.com/wp-content/uploads/2018/09/Categories-of-Personal-Information.pdf> ;
    rdfs:subClassOf dpv:Authenticating ;
    sw:term_status "accepted"@en .

dpv:Sector a rdfs:Class ;
    rdfs:label "Sector"@en ;
    dct:created "2019-04-04"^^xsd:date ;
    dct:date-accepted "2019-04-05"^^xsd:date ;
    dct:description "Used to indicate the sector of a purpose e.g. Agriculture, Advertising (specified e.g. in the form of NACE codes)"@en ;
    sw:term_status "accepted"@en .

dpv:Security a rdfs:Class ;
    rdfs:label "Security"@en ;
    dct:created "2018-12-10"^^xsd:date ;
    dct:creator "Axel Polleres"^^xsd:string,
        "Elmar Kiesling"^^xsd:string,
        "Fajar Ekaputra"^^xsd:string,
        "Harshvardhan J. Pandit"^^xsd:string,
        "Javier Fernandez"^^xsd:string,
        "Simon Steyskal"^^xsd:string ;
    dct:date-accepted "2019-04-05"^^xsd:date ;
    dct:description "Security of data"@en ;
    rdfs:isDefinedBy <https://www.w3.org/community/dpvcg/wiki/Purposes_for_handling_Personal_Data#High-level_categories_.28to-be-discussed.29> ;
    rdfs:subClassOf dpv:Purpose ;
    sw:term_status "accepted"@en .

dpv:SellDataToThirdParties a rdfs:Class ;
    rdfs:label "Sell Data to Third Parties"@en ;
    dct:created "2018-12-10"^^xsd:date ;
    dct:creator "Axel Polleres"^^xsd:string,
        "Elmar Kiesling"^^xsd:string,
        "Fajar Ekaputra"^^xsd:string,
        "Harshvardhan J. Pandit"^^xsd:string,
        "Javier Fernandez"^^xsd:string,
        "Simon Steyskal"^^xsd:string ;
    dct:date-accepted "2019-04-05"^^xsd:date ;
    dct:description "To sell data or information to third parties"@en ;
    rdfs:isDefinedBy <https://www.w3.org/community/dpvcg/wiki/Purposes_for_handling_Personal_Data#High-level_categories_.28to-be-discussed.29> ;
    rdfs:subClassOf dpv:CommercialInterest ;
    sw:term_status "accepted"@en .

dpv:SellInsightsFromData a rdfs:Class ;
    rdfs:label "Sell Insights from Data"@en ;
    dct:created "2018-12-10"^^xsd:date ;
    dct:creator "Axel Polleres"^^xsd:string,
        "Elmar Kiesling"^^xsd:string,
        "Fajar Ekaputra"^^xsd:string,
        "Harshvardhan J. Pandit"^^xsd:string,
        "Javier Fernandez"^^xsd:string,
        "Simon Steyskal"^^xsd:string ;
    dct:date-accepted "2019-04-05"^^xsd:date ;
    dct:description "To sell or commercially provide insights obtained from analysis of data"@en ;
    rdfs:isDefinedBy <https://www.w3.org/community/dpvcg/wiki/Purposes_for_handling_Personal_Data#High-level_categories_.28to-be-discussed.29> ;
    rdfs:subClassOf dpv:CommercialInterest ;
    sw:term_status "accepted"@en .

dpv:SellProductsToDataSubject a rdfs:Class ;
    rdfs:label "Sell Products to Data Subject"@en ;
    dct:created "2018-12-10"^^xsd:date ;
    dct:creator "Axel Polleres"^^xsd:string,
        "Elmar Kiesling"^^xsd:string,
        "Fajar Ekaputra"^^xsd:string,
        "Harshvardhan J. Pandit"^^xsd:string,
        "Javier Fernandez"^^xsd:string,
        "Simon Steyskal"^^xsd:string ;
    dct:date-accepted "2019-04-05"^^xsd:date ;
    dct:description "To sell products or services to the data subject or user"@en ;
    rdfs:isDefinedBy <https://www.w3.org/community/dpvcg/wiki/Purposes_for_handling_Personal_Data#High-level_categories_.28to-be-discussed.29> ;
    rdfs:subClassOf dpv:CommercialInterest ;
    sw:term_status "accepted"@en .

dpv:SellTargettedAdvertisements a rdfs:Class ;
    rdfs:label "Sell Targetted Advertisements"@en ;
    dct:created "2018-12-10"^^xsd:date ;
    dct:creator "Axel Polleres"^^xsd:string,
        "Elmar Kiesling"^^xsd:string,
        "Fajar Ekaputra"^^xsd:string,
        "Harshvardhan J. Pandit"^^xsd:string,
        "Javier Fernandez"^^xsd:string,
        "Simon Steyskal"^^xsd:string ;
    dct:date-accepted "2019-04-05"^^xsd:date ;
    dct:description "To sell or provide targetted advertisements about the user to Third Parties"@en ;
    rdfs:isDefinedBy <https://www.w3.org/community/dpvcg/wiki/Purposes_for_handling_Personal_Data#High-level_categories_.28to-be-discussed.29> ;
    rdfs:subClassOf dpv:CommercialInterest ;
    sw:term_status "accepted"@en .

dpv:ServiceConsumptionBehavior a rdfs:Class ;
    rdfs:label "Service Consumption Behavior"@en ;
    dct:created "2019-11-25"^^xsd:date ;
    dct:creator "Harshvardhan J. Pandit"^^xsd:string,
        "Rudy Jacob"^^xsd:string ;
    dct:date-accepted "2019-11-26"^^xsd:date ;
    dct:description "Information about the consumption of a service by an individual. Examples: time and duration of consumption."@en ;
    rdfs:isDefinedBy "SPECIAL"^^xsd:string ;
    rdfs:subClassOf dpv:Behavioral ;
    sw:term_status "accepted"@en .

dpv:ServiceOptimization a rdfs:Class ;
    rdfs:label "Service Optimization"@en ;
    dct:created "2018-12-10"^^xsd:date ;
    dct:creator "Axel Polleres"^^xsd:string,
        "Elmar Kiesling"^^xsd:string,
        "Fajar Ekaputra"^^xsd:string,
        "Harshvardhan J. Pandit"^^xsd:string,
        "Javier Fernandez"^^xsd:string,
        "Simon Steyskal"^^xsd:string ;
    dct:date-accepted "2019-04-05"^^xsd:date ;
    dct:description "Optimization of service or activity"@en ;
    rdfs:isDefinedBy <https://www.w3.org/community/dpvcg/wiki/Purposes_for_handling_Personal_Data#High-level_categories_.28to-be-discussed.29> ;
    rdfs:subClassOf dpv:Purpose ;
    sw:term_status "accepted"@en .

dpv:ServicePersonalization a rdfs:Class ;
    rdfs:label "Service Personalization"@en ;
    dct:created "2018-12-10"^^xsd:date ;
    dct:creator "Axel Polleres"^^xsd:string,
        "Elmar Kiesling"^^xsd:string,
        "Fajar Ekaputra"^^xsd:string,
        "Harshvardhan J. Pandit"^^xsd:string,
        "Javier Fernandez"^^xsd:string,
        "Simon Steyskal"^^xsd:string ;
    dct:date-accepted "2019-04-05"^^xsd:date ;
    dct:description "Personalization of service or activity for the user"@en ;
    rdfs:isDefinedBy <https://www.w3.org/community/dpvcg/wiki/Purposes_for_handling_Personal_Data#High-level_categories_.28to-be-discussed.29> ;
    rdfs:subClassOf dpv:Purpose ;
    sw:term_status "accepted"@en .

dpv:ServiceProvision a rdfs:Class ;
    rdfs:label "Service Provision"@en ;
    dct:created "2018-12-10"^^xsd:date ;
    dct:creator "Axel Polleres"^^xsd:string,
        "Elmar Kiesling"^^xsd:string,
        "Fajar Ekaputra"^^xsd:string,
        "Harshvardhan J. Pandit"^^xsd:string,
        "Javier Fernandez"^^xsd:string,
        "Simon Steyskal"^^xsd:string ;
    dct:date-accepted "2019-04-05"^^xsd:date ;
    dct:description "Provision of service or activity"@en ;
    rdfs:isDefinedBy <https://www.w3.org/community/dpvcg/wiki/Purposes_for_handling_Personal_Data#High-level_categories_.28to-be-discussed.29> ;
    rdfs:subClassOf dpv:Purpose ;
    sw:term_status "accepted"@en .

dpv:Sexual a rdfs:Class ;
    rdfs:label "Sexual"@en ;
    dct:created "2019-04-04"^^xsd:date ;
    dct:creator "Elmar Kiesling; Harshvardhan J. Pandit"^^xsd:string,
        "Fajar Ekaputra"^^xsd:string ;
    dct:date-accepted "2019-06-04"^^xsd:date ;
    dct:description "Information that describes an individual’s sexual life"@en ;
    rdfs:isDefinedBy <https://enterprivacy.com/wp-content/uploads/2018/09/Categories-of-Personal-Information.pdf> ;
    rdfs:subClassOf dpv:External,
        dpv:SpecialCategoryPersonalData ;
    sw:term_status "accepted"@en .

dpv:SexualHistory a rdfs:Class ;
    rdfs:label "Sexual History"@en ;
    dct:created "2019-04-04"^^xsd:date ;
    dct:creator "Elmar Kiesling; Harshvardhan J. Pandit"^^xsd:string,
        "Fajar Ekaputra"^^xsd:string ;
    dct:date-accepted "2019-06-04"^^xsd:date ;
    dct:description "Information about an individual's sexual history"@en ;
    rdfs:isDefinedBy <https://enterprivacy.com/wp-content/uploads/2018/09/Categories-of-Personal-Information.pdf> ;
    rdfs:subClassOf dpv:Sexual ;
    sw:term_status "accepted"@en .

dpv:SexualPreference a rdfs:Class ;
    rdfs:label "Sexual Preference"@en ;
    dct:created "2019-04-04"^^xsd:date ;
    dct:creator "Elmar Kiesling; Harshvardhan J. Pandit"^^xsd:string,
        "Fajar Ekaputra"^^xsd:string ;
    dct:date-accepted "2019-06-04"^^xsd:date ;
    dct:description "Information about an individual's sexual preferences"@en ;
    rdfs:isDefinedBy <https://enterprivacy.com/wp-content/uploads/2018/09/Categories-of-Personal-Information.pdf> ;
    rdfs:subClassOf dpv:Sexual ;
    sw:term_status "accepted"@en .

dpv:Share a rdfs:Class ;
    rdfs:label "Share"@en ;
    dct:created "2019-04-04"^^xsd:date ;
    dct:date-accepted "2019-05-07"^^xsd:date ;
    dct:description "to give data (or a portion of it) to others"@en ;
    rdfs:isDefinedBy "DPVCG"^^xsd:string ;
    rdfs:subClassOf dpv:Disclose ;
    sw:term_status "accepted"@en .

dpv:Sibling a rdfs:Class ;
    rdfs:label "Sibling"@en ;
    dct:created "2019-04-04"^^xsd:date ;
    dct:creator "Elmar Kiesling; Harshvardhan J. Pandit"^^xsd:string,
        "Fajar Ekaputra"^^xsd:string ;
    dct:date-accepted "2019-06-04"^^xsd:date ;
    dct:description "Information about an individual's sibling(s)."@en ;
    rdfs:isDefinedBy <https://enterprivacy.com/wp-content/uploads/2018/09/Categories-of-Personal-Information.pdf> ;
    rdfs:subClassOf dpv:FamilyStructure ;
    sw:term_status "accepted"@en .

dpv:SkinTone a rdfs:Class ;
    rdfs:label "Skin Tone"@en ;
    dct:created "2019-04-04"^^xsd:date ;
    dct:creator "Elmar Kiesling; Harshvardhan J. Pandit"^^xsd:string,
        "Fajar Ekaputra"^^xsd:string ;
    dct:date-accepted "2019-06-04"^^xsd:date ;
    dct:description "Information about an individual's skin tone"@en ;
    rdfs:isDefinedBy <https://enterprivacy.com/wp-content/uploads/2018/09/Categories-of-Personal-Information.pdf> ;
    rdfs:subClassOf dpv:PhysicalCharacteristic ;
    sw:term_status "accepted"@en .

dpv:Social a rdfs:Class ;
    rdfs:label "Social"@en ;
    dct:created "2019-04-04"^^xsd:date ;
    dct:creator "Elmar Kiesling; Harshvardhan J. Pandit"^^xsd:string,
        "Fajar Ekaputra"^^xsd:string ;
    dct:date-accepted "2019-06-04"^^xsd:date ;
    dct:description "Personal data about the social aspects such as for family, public life, or professional networks."@en ;
    rdfs:isDefinedBy <https://enterprivacy.com/wp-content/uploads/2018/09/Categories-of-Personal-Information.pdf> ;
    rdfs:subClassOf dpv:PersonalDataCategory ;
    sw:term_status "accepted"@en .

dpv:SocialMediaCommunication a rdfs:Class ;
    rdfs:label "Social Media Communication"@en ;
    dct:created "2019-04-04"^^xsd:date ;
    dct:creator "Elmar Kiesling; Harshvardhan J. Pandit"^^xsd:string,
        "Fajar Ekaputra"^^xsd:string ;
    dct:date-accepted "2019-06-04"^^xsd:date ;
    dct:description "Information relating to an individual's social media communication, including the communication itself and metadata."@en ;
    rdfs:isDefinedBy <https://enterprivacy.com/wp-content/uploads/2018/09/Categories-of-Personal-Information.pdf> ;
    rdfs:seeAlso svd:Social ;
    rdfs:subClassOf dpv:Communication ;
    sw:term_status "accepted"@en .

dpv:SocialNetwork a rdfs:Class ;
    rdfs:label "Social Network"@en ;
    dct:created "2019-04-04"^^xsd:date ;
    dct:creator "Elmar Kiesling; Harshvardhan J. Pandit"^^xsd:string,
        "Fajar Ekaputra"^^xsd:string ;
    dct:date-accepted "2019-06-04"^^xsd:date ;
    dct:description "Information about an individual’s friends or connections expressed as a social network"@en ;
    rdfs:isDefinedBy <https://enterprivacy.com/wp-content/uploads/2018/09/Categories-of-Personal-Information.pdf> ;
    rdfs:subClassOf dpv:Social ;
    sw:term_status "accepted"@en .

dpv:SocialStatus a rdfs:Class ;
    rdfs:label "Social Status"@en ;
    dct:created "2019-04-04"^^xsd:date ;
    dct:creator "Elmar Kiesling; Harshvardhan J. Pandit"^^xsd:string,
        "Fajar Ekaputra"^^xsd:string ;
    dct:date-accepted "2019-06-04"^^xsd:date ;
    dct:description "Information about an individual's social status"@en ;
    rdfs:isDefinedBy <https://enterprivacy.com/wp-content/uploads/2018/09/Categories-of-Personal-Information.pdf> ;
    rdfs:subClassOf dpv:PublicLife ;
    sw:term_status "accepted"@en .

dpv:SpecialCategoryPersonalData a rdfs:Class ;
    rdfs:label "Special Category Personal Data"@en ;
    dct:created "2019-04-04"^^xsd:date ;
    dct:creator "Elmar Kiesling; Harshvardhan J. Pandit"^^xsd:string,
        "Fajar Ekaputra"^^xsd:string ;
    dct:date-accepted "2019-05-07"^^xsd:date ;
    dct:description "Special category or personal data as per GDPR Art. 9 (1)"@en ;
    rdfs:comment "trade union membership, which is explicitly included in the taxative listing in GDPR Art. 9 (1), is not covered yet."@en ;
    rdfs:isDefinedBy <https://eur-lex.europa.eu/eli/reg/2016/679/art_9/par_1/oj> ;
    rdfs:subClassOf dpv:PersonalDataCategory ;
    sw:term_status "accepted"@en .

dpv:StaffTraining a rdfs:Class ;
    rdfs:label "Staff Training"@en ;
    dct:created "2019-04-04"^^xsd:date ;
    dct:creator "Axel Polleres"^^xsd:string,
        "Harshvardhan J. Pandit"^^xsd:string,
        "Mark Lizar"^^xsd:string,
        "Rob Brennan"^^xsd:string ;
    dct:date-accepted "2019-04-05"^^xsd:date ;
    dct:description "Practices and policies regarding training of staff members"@en ;
    rdfs:isDefinedBy "DPVCG"^^xsd:string ;
    rdfs:subClassOf dpv:RiskManagementProcedure ;
    sw:term_status "accepted"@en .

dpv:StorageDeletion a rdfs:Class ;
    rdfs:label "Storage Deletion"@en ;
    dct:created "2019-04-04"^^xsd:date ;
    dct:creator "Axel Polleres"^^xsd:string,
        "Harshvardhan J. Pandit"^^xsd:string,
        "Mark Lizar"^^xsd:string,
        "Rob Brennan"^^xsd:string ;
    dct:date-accepted "2019-04-05"^^xsd:date ;
    dct:description "Defines how secure deletion is guaranteed"@en ;
    rdfs:isDefinedBy "DPVCG"^^xsd:string ;
    rdfs:subClassOf dpv:StorageRestriction ;
    sw:term_status "accepted"@en .

dpv:StorageDuration a rdfs:Class ;
    rdfs:label "Storage Duration"@en ;
    dct:created "2019-04-04"^^xsd:date ;
    dct:creator "Axel Polleres"^^xsd:string,
        "Harshvardhan J. Pandit"^^xsd:string,
        "Mark Lizar"^^xsd:string,
        "Rob Brennan"^^xsd:string ;
    dct:date-accepted "2019-04-05"^^xsd:date ;
    dct:description "A duration or temporal entity denoting limitation on storage of personal data"@en ;
    rdfs:isDefinedBy "DPVCG"^^xsd:string ;
    rdfs:subClassOf dpv:StorageRestriction ;
    sw:term_status "accepted"@en .

dpv:StorageLocation a rdfs:Class ;
    rdfs:label "Storage Location"@en ;
    dct:created "2019-04-04"^^xsd:date ;
    dct:creator "Axel Polleres"^^xsd:string,
        "Harshvardhan J. Pandit"^^xsd:string,
        "Mark Lizar"^^xsd:string,
        "Rob Brennan"^^xsd:string ;
    dct:date-accepted "2019-04-05"^^xsd:date ;
    dct:description "Defines a location or goespatial scope, where the data is (physically) stored"@en ;
    rdfs:isDefinedBy "DPVCG"^^xsd:string ;
    rdfs:subClassOf dpv:StorageRestriction ;
    sw:term_status "accepted"@en .

dpv:StorageRestoration a rdfs:Class ;
    rdfs:label "Storage Restoration"@en ;
    dct:created "2019-04-04"^^xsd:date ;
    dct:creator "Axel Polleres"^^xsd:string,
        "Harshvardhan J. Pandit"^^xsd:string,
        "Mark Lizar"^^xsd:string,
        "Rob Brennan"^^xsd:string ;
    dct:date-accepted "2019-04-05"^^xsd:date ;
    dct:description "Regularity and temporal span of data restoration/backup mechanisms that guarantee that data is preserved"@en ;
    rdfs:isDefinedBy "DPVCG"^^xsd:string ;
    rdfs:subClassOf dpv:StorageRestriction ;
    sw:term_status "accepted"@en .

dpv:StorageRestriction a rdfs:Class ;
    rdfs:label "Storage Restriction"@en ;
    dct:created "2019-04-04"^^xsd:date ;
    dct:creator "Axel Polleres"^^xsd:string,
        "Harshvardhan J. Pandit"^^xsd:string,
        "Mark Lizar"^^xsd:string,
        "Rob Brennan"^^xsd:string ;
    dct:date-accepted "2019-04-05"^^xsd:date ;
    dct:description "Restrictions required or followed regarding storage of data"@en ;
    rdfs:isDefinedBy "DPVCG"^^xsd:string ;
    rdfs:subClassOf dpv:TechnicalMeasure ;
    sw:term_status "accepted"@en .

dpv:Store a rdfs:Class ;
    rdfs:label "Store"@en ;
    dct:created "2019-04-04"^^xsd:date ;
    dct:date-accepted "2019-05-07"^^xsd:date ;
    dct:description "to keep data for future use"@en ;
    rdfs:isDefinedBy <https://eur-lex.europa.eu/eli/reg/2016/679/art_4/par_2/oj> ;
    rdfs:subClassOf dpv:Processing ;
    sw:term_status "accepted"@en .

dpv:Structure a rdfs:Class ;
    rdfs:label "Structure"@en ;
    dct:created "2019-04-04"^^xsd:date ;
    dct:date-accepted "2019-05-07"^^xsd:date ;
    dct:description "to arrange data according to a structure"@en ;
    rdfs:isDefinedBy <https://eur-lex.europa.eu/eli/reg/2016/679/art_4/par_2/oj> ;
    rdfs:subClassOf dpv:Organise ;
    sw:term_status "accepted"@en .

dpv:TVViewingBehavior a rdfs:Class ;
    rdfs:label "TV Viewing Behavior"@en ;
    dct:created "2019-11-25"^^xsd:date ;
    dct:creator "Harshvardhan J. Pandit"^^xsd:string,
        "Rudy Jacob"^^xsd:string ;
    dct:date-accepted "2019-11-26"^^xsd:date ;
    dct:description "Information that relates to an individual's TV viewing behavior, such as timestamps of channel change, duration of viewership, content consumed"@en ;
    rdfs:isDefinedBy "SPECIAL"^^xsd:string ;
    rdfs:subClassOf dpv:ServiceConsumptionBehavior ;
    sw:term_status "accepted"@en .

dpv:Tattoo a rdfs:Class ;
    rdfs:label "Tattoo"@en ;
    dct:created "2019-04-04"^^xsd:date ;
    dct:creator "Elmar Kiesling; Harshvardhan J. Pandit"^^xsd:string,
        "Fajar Ekaputra"^^xsd:string ;
    dct:date-accepted "2019-06-04"^^xsd:date ;
    dct:description "Information about an individual's tattoos"@en ;
    rdfs:isDefinedBy <https://enterprivacy.com/wp-content/uploads/2018/09/Categories-of-Personal-Information.pdf> ;
    rdfs:subClassOf dpv:PhysicalCharacteristic ;
    sw:term_status "accepted"@en .

dpv:Tax a rdfs:Class ;
    rdfs:label "Tax"@en ;
    dct:created "2019-04-04"^^xsd:date ;
    dct:creator "Elmar Kiesling; Harshvardhan J. Pandit"^^xsd:string,
        "Fajar Ekaputra"^^xsd:string ;
    dct:date-accepted "2019-06-04"^^xsd:date ;
    dct:description "Information about financial tax e.g. tax records or tax due"@en ;
    rdfs:isDefinedBy <https://enterprivacy.com/wp-content/uploads/2018/09/Categories-of-Personal-Information.pdf> ;
    rdfs:subClassOf dpv:Transactional ;
    sw:term_status "accepted"@en .

dpv:TechnicalMeasure a rdfs:Class ;
    rdfs:label "Technical Measure"@en ;
    dct:created "2019-04-04"^^xsd:date ;
    dct:creator "Axel Polleres"^^xsd:string,
        "Harshvardhan J. Pandit"^^xsd:string,
        "Mark Lizar"^^xsd:string,
        "Rob Brennan"^^xsd:string ;
    dct:date-accepted "2019-04-05"^^xsd:date ;
    dct:description "Technical measures required/followed when processing data of the declared category"@en ;
    rdfs:isDefinedBy "DPVCG"^^xsd:string ;
    rdfs:subClassOf dpv:TechnicalOrganisationalMeasure ;
    sw:term_status "accepted"@en .

dpv:TechnicalOrganisationalMeasure a rdfs:Class ;
    rdfs:label "Technical and Organisational Measure"@en ;
    dct:created "2019-04-04"^^xsd:date ;
    dct:creator "Bud Bruegger"^^xsd:string ;
    dct:date-accepted "2019-04-05"^^xsd:date ;
    dct:description "Technical and organisational measures, for instance security measure, storage restrictions etc. required/followed when processing data of the declared category"@en ;
    rdfs:isDefinedBy "DPVCG"^^xsd:string ;
    sw:term_status "accepted"@en .

dpv:TelephoneNumber a rdfs:Class ;
    rdfs:label "Telephone Number"@en ;
    dct:created "2019-04-04"^^xsd:date ;
    dct:creator "Elmar Kiesling; Harshvardhan J. Pandit"^^xsd:string,
        "Fajar Ekaputra"^^xsd:string ;
    dct:date-accepted "2019-06-04"^^xsd:date ;
    dct:description "Information about an individual's telephone number."@en ;
    rdfs:isDefinedBy <https://enterprivacy.com/wp-content/uploads/2018/09/Categories-of-Personal-Information.pdf> ;
    rdfs:subClassOf dpv:Contact ;
    sw:term_status "accepted"@en .

dpv:ThirdParty a rdfs:Class ;
    rdfs:label "Third Party"@en ;
    dct:created "2019-06-04"^^xsd:date ;
    dct:creator "Harshvardhan J. Pandit"^^xsd:string ;
    dct:date-accepted "2019-06-04"^^xsd:date ;
    dct:description "‘third party’ means a natural or legal person, public authority, agency or body other than the data subject, controller, processor and persons who, under the direct authority of the controller or processor, are authorised to process personal data;"@en ;
    rdfs:isDefinedBy <https://eur-lex.europa.eu/eli/reg/2016/679/art_4/par_10/pnt_g/oj> ;
    rdfs:subClassOf dpv:Recipient ;
    sw:term_status "accepted"@en .

dpv:Thought a rdfs:Class ;
    rdfs:label "Thought"@en ;
    dct:created "2019-04-04"^^xsd:date ;
    dct:creator "Elmar Kiesling; Harshvardhan J. Pandit"^^xsd:string,
        "Fajar Ekaputra"^^xsd:string ;
    dct:date-accepted "2019-06-04"^^xsd:date ;
    dct:description "Information about an individual's thoughts"@en ;
    rdfs:isDefinedBy <https://enterprivacy.com/wp-content/uploads/2018/09/Categories-of-Personal-Information.pdf> ;
    rdfs:subClassOf dpv:KnowledgeBelief ;
    sw:term_status "accepted"@en .

dpv:Tracking a rdfs:Class ;
    rdfs:label "Tracking"@en ;
    dct:created "2019-04-04"^^xsd:date ;
    dct:creator "Elmar Kiesling; Harshvardhan J. Pandit"^^xsd:string,
        "Fajar Ekaputra"^^xsd:string ;
    dct:date-accepted "2019-06-04"^^xsd:date ;
    dct:description "Personal data that can be used to track an individual or used as an identifier e.g. location or email"@en ;
    rdfs:isDefinedBy <https://enterprivacy.com/wp-content/uploads/2018/09/Categories-of-Personal-Information.pdf> ;
    rdfs:subClassOf dpv:PersonalDataCategory ;
    sw:term_status "accepted"@en .

dpv:Transaction a rdfs:Class ;
    rdfs:label "Transaction"@en ;
    dct:created "2019-04-04"^^xsd:date ;
    dct:creator "Elmar Kiesling; Harshvardhan J. Pandit"^^xsd:string,
        "Fajar Ekaputra"^^xsd:string ;
    dct:date-accepted "2019-06-04"^^xsd:date ;
    dct:description "Information about financial transactions e.g. bank transfers"@en ;
    rdfs:isDefinedBy <https://enterprivacy.com/wp-content/uploads/2018/09/Categories-of-Personal-Information.pdf> ;
    rdfs:subClassOf dpv:Transactional ;
    sw:term_status "accepted"@en .

dpv:Transactional a rdfs:Class ;
    rdfs:label "Transactional"@en ;
    dct:created "2019-04-04"^^xsd:date ;
    dct:creator "Elmar Kiesling; Harshvardhan J. Pandit"^^xsd:string,
        "Fajar Ekaputra"^^xsd:string ;
    dct:date-accepted "2019-06-04"^^xsd:date ;
    dct:description "Information about an individual’s purchasing, spending or income"@en ;
    rdfs:isDefinedBy <https://enterprivacy.com/wp-content/uploads/2018/09/Categories-of-Personal-Information.pdf> ;
    rdfs:subClassOf dpv:Financial ;
    sw:term_status "accepted"@en .

dpv:Transfer a rdfs:Class ;
    rdfs:label "Transfer"@en ;
    dct:created "2019-04-04"^^xsd:date ;
    dct:date-accepted "2019-05-07"^^xsd:date ;
    dct:description "to move data from one place to another"@en ;
    rdfs:isDefinedBy <https://www.specialprivacy.eu/vocabs/processing> ;
    rdfs:seeAlso svpr:Transfer ;
    rdfs:subClassOf dpv:Processing ;
    sw:term_status "accepted"@en .

dpv:Transform a rdfs:Class ;
    rdfs:label "Transform"@en ;
    dct:created "2019-04-04"^^xsd:date ;
    dct:date-accepted "2019-05-07"^^xsd:date ;
    dct:description "to change the form or nature of data"@en ;
    rdfs:isDefinedBy "DPVCG"^^xsd:string ;
    rdfs:subClassOf dpv:Processing ;
    sw:term_status "accepted"@en .

dpv:Transmit a rdfs:Class ;
    rdfs:label "Transmit"@en ;
    dct:created "2019-04-04"^^xsd:date ;
    dct:date-accepted "2019-05-07"^^xsd:date ;
    dct:description "to send out data"@en ;
    rdfs:isDefinedBy "DPVCG"^^xsd:string ;
    rdfs:subClassOf dpv:Disclose ;
    sw:term_status "accepted"@en .

dpv:UID a rdfs:Class ;
    rdfs:label "UID"@en ;
    dct:created "2019-04-04"^^xsd:date ;
    dct:creator "Elmar Kiesling; Harshvardhan J. Pandit"^^xsd:string,
        "Fajar Ekaputra"^^xsd:string ;
    dct:date-accepted "2019-06-04"^^xsd:date ;
    dct:description "An unique identifier used to identify an individual."@en ;
    rdfs:isDefinedBy <https://enterprivacy.com/wp-content/uploads/2018/09/Categories-of-Personal-Information.pdf> ;
    rdfs:seeAlso svd:UniqueId ;
    rdfs:subClassOf dpv:Identifying ;
    sw:term_status "accepted"@en .

dpv:Use a rdfs:Class ;
    rdfs:label "Use"@en ;
    dct:created "2019-04-04"^^xsd:date ;
    dct:date-accepted "2019-05-07"^^xsd:date ;
    dct:description "to use data"@en ;
    rdfs:isDefinedBy <https://eur-lex.europa.eu/eli/reg/2016/679/art_4/par_2/oj> ;
    rdfs:subClassOf dpv:Processing ;
    sw:term_status "accepted"@en .

dpv:UserInterfacePersonalisation a rdfs:Class ;
    rdfs:label "User Interface Personalisation"@en ;
    dct:created "2018-12-10"^^xsd:date ;
    dct:creator "Axel Polleres"^^xsd:string,
        "Elmar Kiesling"^^xsd:string,
        "Fajar Ekaputra"^^xsd:string,
        "Harshvardhan J. Pandit"^^xsd:string,
        "Javier Fernandez"^^xsd:string,
        "Simon Steyskal"^^xsd:string ;
    dct:date-accepted "2019-04-05"^^xsd:date ;
    dct:description "Personalisation of interfaces presented to the user"@en ;
    rdfs:isDefinedBy <https://www.w3.org/community/dpvcg/wiki/Purposes_for_handling_Personal_Data#High-level_categories_.28to-be-discussed.29> ;
    rdfs:subClassOf dpv:ServicePersonalization ;
    sw:term_status "accepted"@en .

dpv:Username a rdfs:Class ;
    rdfs:label "Username"@en ;
    dct:created "2019-04-04"^^xsd:date ;
    dct:creator "Elmar Kiesling; Harshvardhan J. Pandit"^^xsd:string,
        "Fajar Ekaputra"^^xsd:string ;
    dct:date-accepted "2019-06-04"^^xsd:date ;
    dct:description "A username used to identify an individual."@en ;
    rdfs:isDefinedBy <https://enterprivacy.com/wp-content/uploads/2018/09/Categories-of-Personal-Information.pdf> ;
    rdfs:subClassOf dpv:Identifying ;
    sw:term_status "accepted"@en .

dpv:VoiceCommunicationRecording a rdfs:Class ;
    rdfs:label "Voice Communication Recording"@en ;
    dct:created "2019-04-04"^^xsd:date ;
    dct:creator "Elmar Kiesling; Harshvardhan J. Pandit"^^xsd:string,
        "Fajar Ekaputra"^^xsd:string ;
    dct:date-accepted "2019-06-04"^^xsd:date ;
    dct:description "Recording of an individual's recorded communication (e.g. telephony, VoIP)"@en ;
    rdfs:comment "ISSUE-23"@en ;
    rdfs:isDefinedBy <https://enterprivacy.com/wp-content/uploads/2018/09/Categories-of-Personal-Information.pdf> ;
    rdfs:subClassOf dpv:Communication ;
    sw:term_status "accepted"@en .

dpv:VoiceMail a rdfs:Class ;
    rdfs:label "Voice Mail"@en ;
    dct:created "2019-04-04"^^xsd:date ;
    dct:creator "Elmar Kiesling; Harshvardhan J. Pandit"^^xsd:string,
        "Fajar Ekaputra"^^xsd:string ;
    dct:date-accepted "2019-06-04"^^xsd:date ;
    dct:description "Information about an individual's voice mail messages."@en ;
    rdfs:isDefinedBy <https://enterprivacy.com/wp-content/uploads/2018/09/Categories-of-Personal-Information.pdf> ;
    rdfs:subClassOf dpv:Communication ;
    sw:term_status "accepted"@en .

dpv:Weight a rdfs:Class ;
    rdfs:label "Weight"@en ;
    dct:created "2019-04-04"^^xsd:date ;
    dct:creator "Elmar Kiesling; Harshvardhan J. Pandit"^^xsd:string,
        "Fajar Ekaputra"^^xsd:string ;
    dct:date-accepted "2019-06-04"^^xsd:date ;
    dct:description "Information about an individual's physical weight"@en ;
    rdfs:isDefinedBy <https://enterprivacy.com/wp-content/uploads/2018/09/Categories-of-Personal-Information.pdf> ;
    rdfs:subClassOf dpv:PhysicalCharacteristic ;
    sw:term_status "accepted"@en .

dpv:WorkHistory a rdfs:Class ;
    rdfs:label "Work History"@en ;
    dct:created "2019-04-04"^^xsd:date ;
    dct:creator "Elmar Kiesling; Harshvardhan J. Pandit"^^xsd:string,
        "Fajar Ekaputra"^^xsd:string ;
    dct:date-accepted "2019-06-04"^^xsd:date ;
    dct:description "Information about an individual's work history in a professional context"@en ;
    rdfs:isDefinedBy <https://enterprivacy.com/wp-content/uploads/2018/09/Categories-of-Personal-Information.pdf> ;
    rdfs:subClassOf dpv:Professional ;
    sw:term_status "accepted"@en .

dpv:consentNotice a rdf:Property ;
    rdfs:label "consent notice"@en ;
    dct:created "2019-04-04"^^xsd:date ;
    dct:creator "Bud Bruegger"^^xsd:string,
        "Harshvardhan J. Pandit"^^xsd:string,
        "Mark Lizar"^^xsd:string ;
    dct:date-accepted "2019-04-05"^^xsd:date ;
    dct:description "Links consent to the notice displayed for requesting consent"@en ;
    rdfs:comment "The actual notice that the Data Subject received to consent to, either a text or link to a document, which should be usable to decide whether the form or consent was compliant to legislation, e.g. documenting how the user has been informed about rights and implications (such as, right to data portability,right to recitffy, right to erasure, right to restrict processing, right to object, rights regarding automated decision making or profiling, processors, third parties, sub-processors, outside-EEA transfers, automated decision-making, or other necessary details of the privacy-policy). Can be TextOrDocumentOrURI."@en ;
    rdfs:domain dpv:Consent ;
    sw:term_status "accepted"@en .

dpv:duration a rdf:Property ;
    rdfs:label "duration"@en ;
    dct:created "2019-04-04"^^xsd:date ;
    dct:creator "Axel Polleres"^^xsd:string,
        "Harshvardhan J. Pandit"^^xsd:string,
        "Mark Lizar"^^xsd:string,
        "Rob Brennan"^^xsd:string ;
    dct:date-accepted "2019-04-05"^^xsd:date ;
    dct:description "Specifies duration for storage of personal data"@en ;
    rdfs:domain dpv:StorageRestriction ;
    rdfs:isDefinedBy "DPVCG"^^xsd:string,
        "SPECIAL"^^xsd:string ;
    rdfs:range dpv:StorageDuration ;
    sw:term_status "accepted"@en .

dpv:expiryCondition a rdf:Property ;
    rdfs:label "expiry condition"@en ;
    dct:created "2019-04-04"^^xsd:date ;
    dct:creator "Bud Bruegger"^^xsd:string,
        "Harshvardhan J. Pandit"^^xsd:string,
        "Mark Lizar"^^xsd:string ;
    dct:date-accepted "2019-04-05"^^xsd:date ;
    dct:description "Specifies the condition or event that determines the expiry of consent"@en ;
    rdfs:comment "Can be TextOrDocumentOrURI"@en ;
    rdfs:domain dpv:Consent ;
    rdfs:subPropertyOf dpv:expiry ;
    sw:term_status "accepted"@en .

dpv:expiryTime a rdf:Property ;
    rdfs:label "expiry time"@en ;
    dct:created "2019-04-04"^^xsd:date ;
    dct:creator "Bud Bruegger"^^xsd:string,
        "Harshvardhan J. Pandit"^^xsd:string,
        "Mark Lizar"^^xsd:string ;
    dct:date-accepted "2019-04-05"^^xsd:date ;
    dct:description "Specifies the expiry time or duration for consent"@en ;
    rdfs:domain dpv:Consent ;
    rdfs:range time:TemporalEntity ;
    rdfs:subPropertyOf dpv:expiry ;
    sw:term_status "accepted"@en .

dpv:hasContext a rdf:Property ;
    rdfs:label "has context"@en ;
    dct:created "2019-04-04"^^xsd:date ;
    dct:date-accepted "2019-04-05"^^xsd:date ;
    dct:description "Restricts a purpose to the specified context(s)"@en ;
    rdfs:domain dpv:Purpose ;
    rdfs:range dpv:Context ;
    sw:term_status "accepted"@en .

dpv:hasDataController a rdf:Property ;
    rdfs:label "has data controller"@en ;
    dct:created "2019-04-04"^^xsd:date ;
    dct:creator "Axel Polleres"^^xsd:string,
        "Bud Bruegger"^^xsd:string,
        "Harshvardhan J. Pandit"^^xsd:string,
        "Javier Ferenandez"^^xsd:string,
        "Mark Lizar"^^xsd:string ;
    dct:date-accepted "2019-04-05"^^xsd:date ;
    dct:description "This property associates a data controller with an instance of legal data handling or consent"@en ;
    rdfs:isDefinedBy "DPVCG"^^xsd:string ;
    rdfs:range dpv:Datacontroller ;
    sw:term_status "accepted"@en .

dpv:hasDataSubject a rdf:Property ;
    rdfs:label "has data subject"@en ;
    dct:created "2019-04-04"^^xsd:date ;
    dct:creator "Axel Polleres"^^xsd:string,
        "Bud Bruegger"^^xsd:string,
        "Harshvardhan J. Pandit"^^xsd:string,
        "Javier Ferenandez"^^xsd:string,
        "Mark Lizar"^^xsd:string ;
    dct:date-accepted "2019-04-05"^^xsd:date ;
    dct:description "This property associates a data subject with an instance of legal data handling or consent"@en ;
    rdfs:isDefinedBy "DPVCG"^^xsd:string ;
    rdfs:range dpv:DataSubject ;
    sw:term_status "accepted"@en .

dpv:hasLegalBasis a rdf:Property ;
    rdfs:label "has legal basis"@en ;
    dct:created "2019-04-04"^^xsd:date ;
    dct:creator "Axel Polleres"^^xsd:string,
        "Javier Ferenandez"^^xsd:string ;
    dct:date-accepted "2019-04-05"^^xsd:date ;
    dct:description "This property associates an instance of legal data handling with its underlying legal basis"@en ;
    rdfs:isDefinedBy "DPVCG"^^xsd:string ;
    rdfs:range dpv:LegalBasis ;
    sw:term_status "accepted"@en .

dpv:hasPersonalDataCategory a rdf:Property ;
    rdfs:label "has personal data category"@en ;
    dct:created "2019-04-04"^^xsd:date ;
    dct:creator "Axel Polleres"^^xsd:string,
        "Bud Bruegger"^^xsd:string,
        "Harshvardhan J. Pandit"^^xsd:string,
        "Javier Ferenandez"^^xsd:string,
        "Mark Lizar"^^xsd:string ;
    dct:date-accepted "2019-04-05"^^xsd:date ;
    dct:description "This property associates a personal data category with an instance of legal data handling or consent"@en ;
    rdfs:isDefinedBy "DPVCG"^^xsd:string,
        "SPECIAL"^^xsd:string ;
    rdfs:range dpv:PersonalDataCategory ;
    sw:term_status "accepted"@en .

dpv:hasProcessing a rdf:Property ;
    rdfs:label "has processing"@en ;
    dct:created "2019-04-04"^^xsd:date ;
    dct:creator "Axel Polleres"^^xsd:string,
        "Bud Bruegger"^^xsd:string,
        "Harshvardhan J. Pandit"^^xsd:string,
        "Javier Ferenandez"^^xsd:string,
        "Mark Lizar"^^xsd:string ;
    dct:date-accepted "2019-04-05"^^xsd:date ;
    dct:description "This property associates a data processing category with an instance of legal data handling or consent"@en ;
    rdfs:isDefinedBy "DPVCG"^^xsd:string,
        "SPECIAL"^^xsd:string ;
    rdfs:range dpv:Processing ;
    sw:term_status "accepted"@en .

dpv:hasPurpose a rdf:Property ;
    rdfs:label "has purpose"@en ;
    dct:created "2019-04-04"^^xsd:date ;
    dct:creator "Axel Polleres"^^xsd:string,
        "Bud Bruegger"^^xsd:string,
        "Harshvardhan J. Pandit"^^xsd:string,
        "Javier Ferenandez"^^xsd:string,
        "Mark Lizar"^^xsd:string ;
    dct:date-accepted "2019-04-05"^^xsd:date ;
    dct:description "This property associates a purpose with an instance of legal data handling or consent"@en ;
    rdfs:isDefinedBy "DPVCG"^^xsd:string,
        "SPECIAL"^^xsd:string ;
    rdfs:range dpv:Purpose ;
    sw:term_status "accepted"@en .

dpv:hasRecipient a rdf:Property ;
    rdfs:label "has recipient"@en ;
    dct:created "2019-04-04"^^xsd:date ;
    dct:creator "Axel Polleres"^^xsd:string,
        "Bud Bruegger"^^xsd:string,
        "Harshvardhan J. Pandit"^^xsd:string,
        "Javier Ferenandez"^^xsd:string,
        "Mark Lizar"^^xsd:string ;
    dct:date-accepted "2019-04-05"^^xsd:date ;
    dct:description "This property associates a recipient with an instance of legal data handling or consent"@en ;
    rdfs:isDefinedBy "DPVCG"^^xsd:string,
        "SPECIAL"^^xsd:string ;
    rdfs:range dpv:Recipient ;
    sw:term_status "accepted"@en .

dpv:hasSector a rdf:Property ;
    rdfs:label "has sector"@en ;
    dct:created "2019-04-04"^^xsd:date ;
    dct:date-accepted "2019-04-05"^^xsd:date ;
    dct:description "Indicates the purpose is associated with activities in the indicated (Economic) Sector(s)"@en ;
    rdfs:domain dpv:Context ;
    rdfs:range dpv:Sector ;
    sw:term_status "accepted"@en .

dpv:hasTechnicalOrganisationalMeasure a rdf:Property ;
    rdfs:label "has technical and organisational measure"@en ;
    dct:created "2019-04-04"^^xsd:date ;
    dct:creator "Axel Polleres"^^xsd:string,
        "Bud Bruegger"^^xsd:string,
        "Harshvardhan J. Pandit"^^xsd:string,
        "Javier Ferenandez"^^xsd:string,
        "Mark Lizar"^^xsd:string ;
    dct:date-accepted "2019-04-05"^^xsd:date ;
    dct:description "This property associates a technical/organisational measure with an instance of legal data handling or consent"@en ;
    rdfs:isDefinedBy "DPVCG"^^xsd:string ;
    rdfs:range dpv:TechnicalOrganisationalMeasure ;
    sw:term_status "accepted"@en .

dpv:innovativeUseOfNewSolutions a rdf:Property ;
    rdfs:label "involves innovative use of new solutions"@en ;
    dct:created "2019-04-04"^^xsd:date ;
    dct:date-accepted "2019-05-07"^^xsd:date ;
    dct:description "Indicates the processing comprises of innovative uses of new or radical solutions"@en ;
    rdfs:comment "e.g. combining fingerprint & face scan for access control. What is concidered new/innovative is of course subject to change over time."@en ;
    rdfs:domain dpv:Processing ;
    rdfs:isDefinedBy "DPVCG"^^xsd:string ;
    rdfs:range xsd:boolean ;
    sw:term_status "accepted"@en .

dpv:isAutomatedDecisionMaking a rdf:Property ;
    rdfs:label "is automated decision making"@en ;
    dct:created "2019-04-04"^^xsd:date ;
    dct:date-accepted "2019-05-07"^^xsd:date ;
    dct:description "Indicates whether the processing comprises of or is part of or results in automated decision making"@en ;
    rdfs:domain dpv:Processing ;
    rdfs:isDefinedBy "DPVCG"^^xsd:string ;
    rdfs:range xsd:boolean ;
    sw:term_status "accepted"@en .

dpv:isEvaluationScoring a rdf:Property ;
    rdfs:label "is evaluation or scoring"@en ;
    dct:created "2019-04-04"^^xsd:date ;
    dct:date-accepted "2019-05-07"^^xsd:date ;
    dct:description "Indicates whether the processing ir part of or results in evaluation or scoring of an individual or their personal data"@en ;
    rdfs:comment "including profiling and predicting,"@en ;
    rdfs:domain dpv:Processing ;
    rdfs:isDefinedBy "DPVCG"^^xsd:string ;
    rdfs:range xsd:boolean ;
    sw:term_status "accepted"@en .

dpv:isExplicit a rdf:Property ;
    rdfs:label "is explicit"@en ;
    dct:created "2019-04-04"^^xsd:date ;
    dct:creator "Bud Bruegger"^^xsd:string,
        "Harshvardhan J. Pandit"^^xsd:string,
        "Mark Lizar"^^xsd:string ;
    dct:date-accepted "2019-04-05"^^xsd:date ;
    dct:description "Indicates consent is explicit as explained in GDPR Article 9.2a and Article 22.2c"@en ;
    rdfs:domain dpv:Consent ;
    rdfs:range xsd:boolean ;
    sw:term_status "accepted"@en .

dpv:isLargeScale a rdf:Property ;
    rdfs:label "is large scale"@en ;
    dct:created "2019-04-04"^^xsd:date ;
    dct:date-accepted "2019-05-07"^^xsd:date ;
    dct:description "Indicates the processing is carried out at large scale in terms of size of data or individuals associated"@en ;
    rdfs:comment """Involves large amounts of personal data or data subjects.
The WP29 recommends that the following factors, in particular, be considered when determining whether the processing is carried out on a large scale (WP29 Guidelines on Data Protection Officer 16/EN WP 243):
a. the number of data subjects concerned, either as a specific number or as a proportion
of the relevant population;
b. the volume of data and/or the range of different data items being processed;
c. the duration, or permanence, of the data processing activity;
d. the geographical extent of the processing activity."""@en ;
    rdfs:domain dpv:Processing ;
    rdfs:isDefinedBy "DPVCG"^^xsd:string ;
    rdfs:range xsd:boolean ;
    sw:term_status "accepted"@en .

dpv:isMatchingCombining a rdf:Property ;
    rdfs:label "is matcing or combining"@en ;
    dct:created "2019-04-04"^^xsd:date ;
    dct:date-accepted "2019-05-07"^^xsd:date ;
    dct:description "Indicates whether the processing comprises of matching or combining existing data"@en ;
    rdfs:comment "originating from two or more data processing operations performed for different purposes and/or by different data controllers in a way that would exceed the reasonable expectations of the data subject (WP29 Opinion on Purpose limitation 13/EN WP 203, p.24).  For instance Integration/Enrichment with other data (not necessarily personal only)"@en ;
    rdfs:domain dpv:Processing ;
    rdfs:isDefinedBy "DPVCG"^^xsd:string ;
    rdfs:range xsd:boolean ;
    sw:term_status "accepted"@en .

dpv:isSystematicMonitoring a rdf:Property ;
    rdfs:label "is systematic or monitoring"@en ;
    dct:created "2019-04-04"^^xsd:date ;
    dct:date-accepted "2019-05-07"^^xsd:date ;
    dct:description "Indicates whether the processing comprises of systematic monitoring of data subjects or their personal data"@en ;
    rdfs:domain dpv:Processing ;
    rdfs:isDefinedBy "DPVCG"^^xsd:string ;
    rdfs:range xsd:boolean ;
    sw:term_status "accepted"@en .

dpv:location a rdf:Property ;
    rdfs:label "location"@en ;
    dct:created "2019-04-04"^^xsd:date ;
    dct:creator "Axel Polleres"^^xsd:string,
        "Harshvardhan J. Pandit"^^xsd:string,
        "Mark Lizar"^^xsd:string,
        "Rob Brennan"^^xsd:string ;
    dct:date-accepted "2019-04-05"^^xsd:date ;
    dct:description "Specifies location for storage of personal data"@en ;
    rdfs:domain dpv:StorageRestriction ;
    rdfs:isDefinedBy "DPVCG"^^xsd:string,
        "SPECIAL"^^xsd:string ;
    rdfs:range dpv:StorageLocation ;
    sw:term_status "accepted"@en .

dpv:measureImplementedBy a rdf:Property ;
    rdfs:label "measure implemented by"@en ;
    dct:created "2019-04-23"^^xsd:date ;
    dct:creator "Axel Polleres"^^xsd:string ;
    dct:date-accepted "2019-05-07"^^xsd:date ;
    dct:description "a generic ObjectProperty to describe how the measure is implemented.  For the values of this property we either allow a blank node with a single rdfs:comment to describe the measure, or a URI to a standard or best practice followed, i.e. a well-known identifier for that standard or a URL where the respective document describes the standard."@en ;
    rdfs:domain dpv:TechnicalOrganisationalMeasure ;
    rdfs:isDefinedBy "DPVCG"^^xsd:string ;
    rdfs:range rdfs:Resource ;
    sw:term_status "accepted"@en .

dpv:provisionBy a rdf:Property ;
    rdfs:label "provision by"@en ;
    dct:created "2019-04-04"^^xsd:date ;
    dct:creator "Bud Bruegger"^^xsd:string,
        "Harshvardhan J. Pandit"^^xsd:string,
        "Mark Lizar"^^xsd:string ;
    dct:date-accepted "2019-04-05"^^xsd:date ;
    dct:description "Specifies the entity that provisioned or provided consent"@en ;
    rdfs:comment "Normally this would be the dataSubject, but in some exceptional cases, the consent might be given on behalf by someone else, e.g. parents of minors."@en ;
    rdfs:domain dpv:Consent ;
    rdfs:range dpv:LegalEntity ;
    sw:term_status "accepted"@en .

dpv:provisionByJustification a rdf:Property ;
    rdfs:label "provision by justification"@en ;
    dct:created "2019-04-04"^^xsd:date ;
    dct:creator "Bud Bruegger"^^xsd:string,
        "Harshvardhan J. Pandit"^^xsd:string,
        "Mark Lizar"^^xsd:string ;
    dct:date-accepted "2019-04-05"^^xsd:date ;
    dct:description "Specifies the justification for entity providing consent"@en ;
    rdfs:comment "This field can be used to proivde a justification why the provision was provided by another DataSubject or legal entity,  e.g. declariing the relationship (parent, guardian), in combination with the field provisionBy"@en ;
    rdfs:domain dpv:Consent ;
    sw:term_status "accepted"@en .

dpv:provisionMethod a rdf:Property ;
    rdfs:label "provision method"@en ;
    dct:created "2019-04-04"^^xsd:date ;
    dct:creator "Bud Bruegger"^^xsd:string,
        "Harshvardhan J. Pandit"^^xsd:string,
        "Mark Lizar"^^xsd:string ;
    dct:date-accepted "2019-04-05"^^xsd:date ;
    dct:description "Specifies the method by which consent was provisioned or provided"@en ;
    rdfs:comment "Can be used to record information of how consent was provided e.g. by a click to a form, in writing, etc., by logging into a system and confirm per email, or with some additional authentication, etc."@en ;
    rdfs:domain dpv:Consent ;
    sw:term_status "accepted"@en .

dpv:provisionTime a rdf:Property ;
    rdfs:label "provision time"@en ;
    dct:created "2019-04-04"^^xsd:date ;
    dct:creator "Bud Bruegger"^^xsd:string,
        "Harshvardhan J. Pandit"^^xsd:string,
        "Mark Lizar"^^xsd:string ;
    dct:date-accepted "2019-04-05"^^xsd:date ;
    dct:description "Specifies the instant in time when consent was given"@en ;
    rdfs:domain dpv:Consent ;
    rdfs:range time:Instant ;
    sw:term_status "accepted"@en .

dpv:storage a rdf:Property ;
    rdfs:label "storage"@en ;
    dct:created "2019-04-04"^^xsd:date ;
    dct:creator "Axel Polleres"^^xsd:string,
        "Harshvardhan J. Pandit"^^xsd:string,
        "Mark Lizar"^^xsd:string,
        "Rob Brennan"^^xsd:string ;
    dct:date-accepted "2019-04-05"^^xsd:date ;
    dct:description "Specifies restriction on the storage of personal data"@en ;
    rdfs:domain dpv:TechnicalOrganisationalMeasure ;
    rdfs:isDefinedBy "DPVCG"^^xsd:string,
        "SPECIAL"^^xsd:string ;
    rdfs:range dpv:StorageRestriction ;
    sw:term_status "accepted"@en .

dpv:withdrawalBy a rdf:Property ;
    rdfs:label "withdrawal by"@en ;
    dct:created "2019-04-04"^^xsd:date ;
    dct:creator "Bud Bruegger"^^xsd:string,
        "Harshvardhan J. Pandit"^^xsd:string,
        "Mark Lizar"^^xsd:string ;
    dct:date-accepted "2019-04-05"^^xsd:date ;
    dct:description "Specifies the entity that withdrew consent"@en ;
    rdfs:comment "Normally this would be the dataSubject, but in some exceptional cases, the consent might be withdraawn on behalf by someone else, e.g. parents of minors."@en ;
    rdfs:domain dpv:Consent ;
    rdfs:range dpv:LegalEntity ;
    sw:term_status "accepted"@en .

dpv:withdrawalByJustification a rdf:Property ;
    rdfs:label "withdrawal by justification"@en ;
    dct:created "2019-04-04"^^xsd:date ;
    dct:creator "Bud Bruegger"^^xsd:string,
        "Harshvardhan J. Pandit"^^xsd:string,
        "Mark Lizar"^^xsd:string ;
    dct:date-accepted "2019-04-05"^^xsd:date ;
    dct:description "Specifies the justification for entity withdrawing consent"@en ;
    rdfs:comment "This field can be used to proivde a justification why the weithdrawal was done by another DataSubject or legal entity, e.g. declariing the relationship (parent, guardian), in combination with the field withdrawalBy"@en ;
    rdfs:domain dpv:Consent ;
    sw:term_status "accepted"@en .

dpv:withdrawalMethod a rdf:Property ;
    rdfs:label "withdrawal method"@en ;
    dct:created "2019-04-04"^^xsd:date ;
    dct:creator "Bud Bruegger"^^xsd:string,
        "Harshvardhan J. Pandit"^^xsd:string,
        "Mark Lizar"^^xsd:string ;
    dct:date-accepted "2019-04-05"^^xsd:date ;
    dct:description "Specifries the method by which consent can be/has been withdrawn"@en ;
    rdfs:comment "Can be used to record information of how to withdraw consent, e.g. by a click to a form, in writing, etc., by logging into a system and confirm per email, or with some additional authentication, etc."@en ;
    rdfs:domain dpv:Consent ;
    sw:term_status "accepted"@en .

dpv:withdrawalTime a rdf:Property ;
    rdfs:label "withdrawal time"@en ;
    dct:created "2019-04-04"^^xsd:date ;
    dct:creator "Bud Bruegger"^^xsd:string,
        "Harshvardhan J. Pandit"^^xsd:string,
        "Mark Lizar"^^xsd:string ;
    dct:date-accepted "2019-04-05"^^xsd:date ;
    dct:description "Specifies the instant in time when consent was withdrawn"@en ;
    rdfs:domain dpv:Consent ;
    rdfs:range time:Instant ;
    sw:term_status "accepted"@en .

<https://w3.org/ns/dpv> a owl:Ontology ;
    dct:abstract "The Data Privacy Vocabulary provides terms (classes and properties) to annotate and categorize instances of legally compliant personal data handling according to the EU General Data Protection Regulation. This scope could be extended by later versions to other data and privacy protection regulations. The vocabulary provides terms to describe which personal data Categories are undergoing a specified kind of processing by a specific data controller and/or transferred to some recipient for a particular purpose , based on a specific legal ground (e.g. consent, or other legal grounds such as legitimate interest, etc.), with specified technical and organisational measures and restrictions (e.g. storage locations and storage durations) in place."@en ;
    dct:contributor "Bert Bos",
        "Bud Bruegger",
        "Elmar Kiesling",
        "Eva Schlehahn",
        "Fajar J. Ekaputra",
        "Javier D. Fernández",
        "Mark Lizar",
        "Ramisa Gachpaz Hamed",
        "Rigo Wenning",
        "Rob Brennan",
        "Simon Steyskal" ;
    dct:created "2019-06-18"^^xsd:date ;
    dct:creator "Axel Polleres",
        "Harshvardhan J. Pandit" ;
    dct:description "The Data Privacy Vocabulary provides terms (classes and properties) to annotate and categorize instances of legally compliant personal data handling. These terms are intended to annotate Legal Personal Data Handling in a machine-readable fashion, by specifying which personal data categories are undergoing a specific kind of processing, by a specific data controller and/or shared with some recipient for a particular purpose , based on a specific legal ground (e.g. consent or legitimate interest), with specific technical and organisational measures and restrictions (e.g. storage location and storage duration) in place."@en ;
    dct:source <https://www.w3.org/community/dpvcg/> ;
    dct:title "Data Privacy Vocabulary"@en ;
    ns1:preferredNamespacePrefix "dpv" ;
    ns1:preferredNamespaceUri "https://w3.org/ns/dpv"^^xsd:string ;
    owl:versionInfo "0.1"^^xsd:string .

dpv:expiry a rdf:Property ;
    rdfs:label "expiry"@en ;
    dct:created "2019-04-04"^^xsd:date ;
    dct:creator "Bud Bruegger"^^xsd:string,
        "Harshvardhan J. Pandit"^^xsd:string,
        "Mark Lizar"^^xsd:string ;
    dct:date-accepted "2019-04-05"^^xsd:date ;
    dct:description "Generic property specifying when or under which condition(s) the consent will expire"@en ;
    rdfs:domain dpv:Consent ;
    sw:term_status "accepted"@en .

