@prefix dct: <http://purl.org/dc/terms/> .
@prefix dpv: <https://w3id.org/dpv#> .
@prefix owl: <http://www.w3.org/2002/07/owl#> .
@prefix rdfs: <http://www.w3.org/2000/01/rdf-schema#> .
@prefix schema: <https://schema.org/> .
@prefix skos: <http://www.w3.org/2004/02/skos/core#> .
@prefix sw: <http://www.w3.org/2003/06/sw-vocab-status/ns#> .
@prefix tech: <https://w3id.org/dpv/tech#> .
@prefix vann: <http://purl.org/vocab/vann/> .
@prefix xsd: <http://www.w3.org/2001/XMLSchema#> .

tech:CovertSurveillanceTechnology a rdfs:Class,
        skos:Concept,
        dpv:Technology ;
    dct:contributor "Harshvardhan J. Pandit" ;
    dct:created "2022-06-15"^^xsd:date ;
    rdfs:isDefinedBy tech: ;
    sw:term_status "accepted"@en ;
    skos:broader tech:SurveillanceTechnology ;
    skos:definition "Surveillance that is covert i.e. invisible or non-apparent or implicit"@en ;
    skos:inScheme tech:surveillance-classes ;
    skos:prefLabel "Covert SurveillanceTechnology"@en ;
    skos:scopeNote "For example, a web resource that performs tracking in the background"@en .

tech:OvertSurveillanceTechnology a rdfs:Class,
        skos:Concept,
        dpv:Technology ;
    dct:contributor "Harshvardhan J. Pandit" ;
    dct:created "2022-06-15"^^xsd:date ;
    rdfs:isDefinedBy tech: ;
    sw:term_status "accepted"@en ;
    skos:broader tech:SurveillanceTechnology ;
    skos:definition "Surveillance that is overt i.e. visible or apparent or explicit"@en ;
    skos:inScheme tech:surveillance-classes ;
    skos:prefLabel "Overt Surveillance Technology"@en ;
    skos:scopeNote "For example, a CCTV with a notice"@en .

<https://w3id.org/dpv/tech> a owl:Ontology ;
    dct:conformsTo "http://www.w3.org/2000/01/rdf-schema",
        "http://www.w3.org/2004/02/skos/core" ;
    dct:contributor "Harshvardhan J. Pandit" ;
    dct:created "2022-06-15"@en ;
    dct:creator "Georg P Krog"@en,
        "Harshvardhan J. Pandit"@en,
        "Julian Flake"@en,
        "Paul Ryan"@en ;
    dct:description "Extension to the Data Privacy Vocabulary (DPV) providing concepts for representing information about technologies and its provision"@en ;
    dct:identifier "https://w3id.org/dpv/tech" ;
    dct:license <https://www.w3.org/copyright/document-license-2023/> ;
    dct:modified "2024-01-01"@en ;
    dct:title "Technology Concepts"@en ;
    vann:preferredNamespacePrefix "tech" ;
    vann:preferredNamespaceUri "https://w3id.org/dpv/tech#" ;
    schema:version "0.8.2" .

tech:SurveillanceTechnology skos:narrower tech:CovertSurveillanceTechnology,
        tech:OvertSurveillanceTechnology .

tech:surveillance-classes a skos:ConceptScheme .

