@prefix dct: <http://purl.org/dc/terms/> .
@prefix dpv: <https://w3id.org/dpv#> .
@prefix owl: <http://www.w3.org/2002/07/owl#> .
@prefix rdfs: <http://www.w3.org/2000/01/rdf-schema#> .
@prefix schema: <https://schema.org/> .
@prefix skos: <http://www.w3.org/2004/02/skos/core#> .
@prefix sw: <http://www.w3.org/2003/06/sw-vocab-status/ns#> .
@prefix tech: <https://w3id.org/dpv/tech#> .
@prefix vann: <http://purl.org/vocab/vann/> .
@prefix xsd: <http://www.w3.org/2001/XMLSchema#> .

tech:Cookie a rdfs:Class,
        owl:Class,
        dpv:Technology ;
    dct:contributor "Harshvardhan J. Pandit" ;
    dct:created "2022-06-15"^^xsd:date ;
    rdfs:isDefinedBy tech: ;
    rdfs:subClassOf tech:LocalStorage ;
    sw:term_status "accepted"@en ;
    skos:definition "A HTTP or web or internet cookie"@en ;
    skos:prefLabel "Cookie"@en .

tech:Database a rdfs:Class,
        owl:Class,
        dpv:Technology ;
    dct:contributor "Harshvardhan J. Pandit" ;
    dct:created "2022-06-15"^^xsd:date ;
    rdfs:isDefinedBy tech: ;
    rdfs:subClassOf tech:DataStorageTechnology ;
    sw:term_status "accepted"@en ;
    skos:definition "A database, database management system (DBMS), or application database"@en ;
    skos:prefLabel "Database"@en .

tech:FileSystem a rdfs:Class,
        owl:Class,
        dpv:Technology ;
    dct:contributor "Harshvardhan J. Pandit" ;
    dct:created "2022-06-15"^^xsd:date ;
    rdfs:isDefinedBy tech: ;
    rdfs:subClassOf tech:DataStorageTechnology ;
    sw:term_status "accepted"@en ;
    skos:definition "A data storage and retrieval interface provided by an operating system"@en ;
    skos:prefLabel "File System"@en .

tech:IdentityManagementTechnology a rdfs:Class,
        owl:Class,
        dpv:Technology ;
    dct:contributor "Harshvardhan J. Pandit" ;
    dct:created "2022-06-15"^^xsd:date ;
    rdfs:isDefinedBy tech: ;
    rdfs:subClassOf tech:IdentityTechnology,
        tech:ManagementTechnology ;
    rdfs:superClassOf tech:IdentityWallet ;
    sw:term_status "accepted"@en ;
    skos:definition "Technologies providing identity provision, verification, management, and governance"@en ;
    skos:prefLabel "Identity Management Technology"@en .

tech:IdentityWallet a rdfs:Class,
        owl:Class,
        dpv:Technology ;
    dct:contributor "Harshvardhan J. Pandit" ;
    dct:created "2022-06-15"^^xsd:date ;
    rdfs:isDefinedBy tech: ;
    rdfs:subClassOf tech:DataStorageTechnology,
        tech:IdentityManagementTechnology ;
    sw:term_status "accepted"@en ;
    skos:definition "product and service that allows the user to store identity data, credentials and attributes linked to her/his identity, to provide them to relying parties on request and to use them for authentication, online and offline, and to create qualified electronic signatures and seals"@en ;
    skos:prefLabel "Identity Wallet"@en .

tech:PersonalInformationManagementSystem a rdfs:Class,
        owl:Class,
        dpv:Technology ;
    dct:contributor "Harshvardhan J. Pandit" ;
    dct:created "2022-06-15"^^xsd:date ;
    rdfs:isDefinedBy tech: ;
    rdfs:subClassOf tech:DataManagementTechnology ;
    sw:term_status "accepted"@en ;
    skos:definition "A PIMS is a system that helps to give individuals more control over their personal data by managing their personal data in secure, on-premises or online storage systems and sharing it when and with whomever they choose"@en ;
    skos:prefLabel "Personal Information Management System"@en .

tech:SmartphoneApplication a rdfs:Class,
        owl:Class,
        dpv:Technology ;
    dct:contributor "Harshvardhan J. Pandit" ;
    dct:created "2022-06-15"^^xsd:date ;
    rdfs:isDefinedBy tech: ;
    rdfs:subClassOf tech:Application ;
    sw:term_status "accepted"@en ;
    skos:definition "A computing or digital program on a smartphone device"@en ;
    skos:prefLabel "Smartphone Application"@en .

<https://w3id.org/dpv/tech> a owl:Ontology ;
    dct:conformsTo <http://www.w3.org/2002/07/owl>,
        "http://www.w3.org/2000/01/rdf-schema",
        "http://www.w3.org/2004/02/skos/core" ;
    dct:contributor "Harshvardhan J. Pandit" ;
    dct:created "2022-06-15"@en ;
    dct:creator "Georg P Krog"@en,
        "Harshvardhan J. Pandit"@en,
        "Julian Flake"@en,
        "Paul Ryan"@en ;
    dct:description "Extension to the Data Privacy Vocabulary (DPV) providing concepts for representing information about technologies and its provision"@en ;
    dct:hasVersion <https://w3id.org/dpv/tech> ;
    dct:identifier "https://w3id.org/dpv/tech" ;
    dct:license <https://www.w3.org/copyright/document-license-2023/> ;
    dct:modified "2024-01-01"@en ;
    dct:title "Technology Concepts"@en ;
    vann:preferredNamespacePrefix "tech" ;
    vann:preferredNamespaceUri "https://w3id.org/dpv/tech#" ;
    schema:version "0.8.2" .

tech:Application rdfs:superClassOf tech:SmartphoneApplication .

tech:DataManagementTechnology rdfs:superClassOf tech:PersonalInformationManagementSystem .

tech:IdentityTechnology rdfs:superClassOf tech:IdentityManagementTechnology .

tech:LocalStorage rdfs:superClassOf tech:Cookie .

tech:ManagementTechnology rdfs:superClassOf tech:IdentityManagementTechnology .

tech:DataStorageTechnology rdfs:superClassOf tech:Database,
        tech:FileSystem,
        tech:IdentityWallet .

