@prefix bibo: <http://purl.org/ontology/bibo/> .
@prefix dcam: <http://purl.org/dc/dcam/> .
@prefix dct: <http://purl.org/dc/terms/> .
@prefix dex: <https://w3id.org/dpv/examples#> .
@prefix dpv: <https://w3id.org/dpv#> .
@prefix foaf: <http://xmlns.com/foaf/0.1/> .
@prefix org: <http://www.w3.org/ns/org#> .
@prefix owl: <http://www.w3.org/2002/07/owl#> .
@prefix profile: <http://www.w3.org/ns/dx/prof/> .
@prefix rdf: <http://www.w3.org/1999/02/22-rdf-syntax-ns#> .
@prefix rdfs: <http://www.w3.org/2000/01/rdf-schema#> .
@prefix role: <http://www.w3.org/ns/dx/prof/role/> .
@prefix schema: <https://schema.org/> .
@prefix scoro: <http://purl.org/spar/scoro/> .
@prefix skos: <http://www.w3.org/2004/02/skos/core#> .
@prefix sw: <http://www.w3.org/2003/06/sw-vocab-status/ns#> .
@prefix vann: <http://purl.org/vocab/vann/> .
@prefix xsd: <http://www.w3.org/2001/XMLSchema#> .

dpv:AcceptableRule a rdfs:Class,
        skos:Concept,
        dpv:Rule ;
    dct:contributor _:person-arthit-suriyawongkul,
        _:person-beatriz-esteves,
        _:person-delaram-golpayegani,
        _:person-georg-p-krog,
        _:person-harshvardhan-j-pandit,
        _:person-julian-flake,
        _:person-paul-ryan ;
    dct:created "2025-06-19"^^xsd:date ;
    rdfs:isDefinedBy dpv: ;
    sw:term_status "accepted"@en ;
    skos:broader dpv:Rule ;
    skos:definition "A rule that is acceptable where it is either desirable if it occurs or it is not unacceptable if it does"@en ;
    skos:inScheme dpv:rules-classes ;
    skos:prefLabel "Acceptable Rule"@en ;
    skos:scopeNote "Acceptable is a subjective concept that enables distinguishing with \"unacceptable\". By itself it does not signal any permission or obligation - for which further specific concepts are defined"@en .

dpv:Deterrence a rdfs:Class,
        skos:Concept,
        dpv:Rule ;
    dct:contributor _:person-arthit-suriyawongkul,
        _:person-beatriz-esteves,
        _:person-delaram-golpayegani,
        _:person-georg-p-krog,
        _:person-harshvardhan-j-pandit,
        _:person-julian-flake,
        _:person-paul-ryan ;
    dct:created "2025-06-19"^^xsd:date ;
    rdfs:isDefinedBy dpv: ;
    sw:term_status "accepted"@en ;
    skos:broader dpv:UnacceptableRule ;
    skos:definition "A rule describing a deterrence for performing an activity"@en ;
    skos:inScheme dpv:rules-classes ;
    skos:prefLabel "Deterrence"@en ;
    skos:scopeNote "Deterrences are aligned with the term SHOULD NOT in RFC2119 where specified activities should be avoided from being carried out but are not prohibitions"@en .

dpv:DeterrenceFollowed a rdfs:Class,
        skos:Concept,
        dpv:RuleFulfilmentStatus ;
    dct:contributor _:person-beatriz-esteves,
        _:person-georg-p-krog,
        _:person-harshvardhan-j-pandit,
        _:person-julian-flake ;
    dct:created "2025-08-06"^^xsd:date ;
    rdfs:isDefinedBy dpv: ;
    sw:term_status "accepted"@en ;
    skos:broader dpv:RuleFulfilled ;
    skos:definition "Status indicating a deterrence has been followed i.e. the activity stated as being deterred has not been carried out"@en ;
    skos:inScheme dpv:rules-classes ;
    skos:prefLabel "Deterrence Followed"@en .

dpv:DeterrenceNotFollowed a rdfs:Class,
        skos:Concept,
        dpv:RuleFulfilmentStatus ;
    dct:contributor _:person-beatriz-esteves,
        _:person-georg-p-krog,
        _:person-harshvardhan-j-pandit,
        _:person-julian-flake ;
    dct:created "2025-08-06"^^xsd:date ;
    rdfs:isDefinedBy dpv: ;
    sw:term_status "accepted"@en ;
    skos:broader dpv:RuleUnfulfilled ;
    skos:definition "Status indicating a deterrence has not been followed i.e. the activity stated as being deterred has been carried out"@en ;
    skos:inScheme dpv:rules-classes ;
    skos:prefLabel "Deterrence Not Followed"@en .

dpv:Obligation a rdfs:Class,
        skos:Concept,
        dpv:Rule ;
    dct:contributor _:person-arthit-suriyawongkul,
        _:person-beatriz-esteves,
        _:person-delaram-golpayegani,
        _:person-georg-p-krog,
        _:person-harshvardhan-j-pandit,
        _:person-julian-flake,
        _:person-paul-ryan ;
    dct:created "2022-10-19"^^xsd:date ;
    dct:modified "2025-06-19"^^xsd:date ;
    rdfs:isDefinedBy dpv: ;
    sw:term_status "modified"@en ;
    skos:broader dpv:AcceptableRule ;
    skos:definition "A rule describing an obligation for performing an activity"@en ;
    skos:inScheme dpv:rules-classes ;
    skos:prefLabel "Obligation"@en ;
    skos:scopeNote "Obligations are aligned with the term MUST in RFC2119 where specified activities are mandatory to be carried out"@en .

dpv:ObligationFulfilled a rdfs:Class,
        skos:Concept,
        dpv:RuleFulfilmentStatus ;
    dct:contributor _:person-harshvardhan-j-pandit ;
    dct:created "2024-09-10"^^xsd:date ;
    rdfs:isDefinedBy dpv: ;
    sw:term_status "accepted"@en ;
    skos:broader dpv:RuleFulfilled ;
    skos:definition "Status indicating an obligation has been fulfilled i.e. the activity stated as being required to be carried out has been successfully completed"@en ;
    skos:inScheme dpv:rules-classes ;
    skos:prefLabel "Obligation Fulfilled"@en .

dpv:ObligationUnfulfilled a rdfs:Class,
        skos:Concept,
        dpv:RuleFulfilmentStatus ;
    dct:contributor _:person-harshvardhan-j-pandit ;
    dct:created "2024-09-10"^^xsd:date ;
    rdfs:isDefinedBy dpv: ;
    sw:term_status "accepted"@en ;
    skos:broader dpv:RuleUnfulfilled ;
    skos:definition "Status indicating an obligation has not been fulfilled i.e. the activity stated as being required to be carried out has not been carried out but this is not considered as a violation e.g. there is still time to conduct the activity"@en ;
    skos:inScheme dpv:rules-classes ;
    skos:prefLabel "Obligation Unfulfilled"@en .

dpv:ObligationViolated a rdfs:Class,
        skos:Concept,
        dpv:RuleFulfilmentStatus ;
    dct:contributor _:person-harshvardhan-j-pandit ;
    dct:created "2024-09-10"^^xsd:date ;
    rdfs:isDefinedBy dpv: ;
    sw:term_status "accepted"@en ;
    skos:broader dpv:RuleViolated ;
    skos:definition "Status indicating an obligation has been violated i.e. the activity stated as being required to be carried out has not been carried out and this is considered as a violation i.e. the activity can no longer be carried out to fulfil the obligation"@en ;
    skos:inScheme dpv:rules-classes ;
    skos:prefLabel "Obligation Violated"@en .

dpv:Permission a rdfs:Class,
        skos:Concept,
        dpv:Rule ;
    dct:contributor _:person-arthit-suriyawongkul,
        _:person-beatriz-esteves,
        _:person-delaram-golpayegani,
        _:person-georg-p-krog,
        _:person-harshvardhan-j-pandit,
        _:person-julian-flake,
        _:person-paul-ryan ;
    dct:created "2022-10-19"^^xsd:date ;
    dct:modified "2025-06-19"^^xsd:date ;
    vann:example dex:E0028,
        dex:E0066 ;
    rdfs:isDefinedBy dpv: ;
    sw:term_status "modified"@en ;
    skos:broader dpv:AcceptableRule ;
    skos:definition "A rule describing a permission to perform an activity"@en ;
    skos:inScheme dpv:rules-classes ;
    skos:prefLabel "Permission"@en ;
    skos:scopeNote "Permissions are aligned with the term MAY in RFC2119 where specified activities may or may not be carried out"@en .

dpv:PermissionNotUtilised a rdfs:Class,
        skos:Concept,
        dpv:RuleFulfilmentStatus ;
    dct:contributor _:person-harshvardhan-j-pandit ;
    dct:created "2024-09-10"^^xsd:date ;
    rdfs:isDefinedBy dpv: ;
    sw:term_status "accepted"@en ;
    skos:broader dpv:RuleFulfilled ;
    skos:definition "Status indicating a permission has not been utilised i.e. the activity stated as being permitted has not been carried out"@en ;
    skos:inScheme dpv:rules-classes ;
    skos:prefLabel "Permission Not Utilised"@en .

dpv:PermissionUtilised a rdfs:Class,
        skos:Concept,
        dpv:RuleFulfilmentStatus ;
    dct:contributor _:person-harshvardhan-j-pandit ;
    dct:created "2024-09-10"^^xsd:date ;
    rdfs:isDefinedBy dpv: ;
    sw:term_status "accepted"@en ;
    skos:broader dpv:RuleFulfilled ;
    skos:definition "Status indicating a permission has been utilised i.e. the activity stated as being permitted has been carried out"@en ;
    skos:inScheme dpv:rules-classes ;
    skos:prefLabel "Permission Utilised"@en .

dpv:Prohibition a rdfs:Class,
        skos:Concept,
        dpv:Rule ;
    dct:contributor _:person-arthit-suriyawongkul,
        _:person-beatriz-esteves,
        _:person-delaram-golpayegani,
        _:person-georg-p-krog,
        _:person-harshvardhan-j-pandit,
        _:person-julian-flake,
        _:person-paul-ryan ;
    dct:created "2022-10-19"^^xsd:date ;
    dct:modified "2025-06-19"^^xsd:date ;
    vann:example dex:E0029,
        dex:E0066 ;
    rdfs:isDefinedBy dpv: ;
    sw:term_status "modified"@en ;
    skos:broader dpv:UnacceptableRule ;
    skos:definition "A rule describing a prohibition to perform an activity"@en ;
    skos:inScheme dpv:rules-classes ;
    skos:prefLabel "Prohibition"@en ;
    skos:scopeNote "Prohibitions are aligned with the term MUST NOT in RFC2119 where specified activities are prohibited from being carried out"@en .

dpv:ProhibitionUnviolated a rdfs:Class,
        skos:Concept,
        dpv:RuleFulfilmentStatus ;
    dct:contributor _:person-beatriz-esteves,
        _:person-georg-p-krog,
        _:person-harshvardhan-j-pandit,
        _:person-julian-flake ;
    dct:created "2024-09-10"^^xsd:date ;
    dct:modified "2025-08-06"^^xsd:date ;
    rdfs:isDefinedBy dpv: ;
    sw:term_status "modified"@en ;
    skos:broader dpv:RuleFulfilled ;
    skos:definition "Status indicating a prohibition has not been violated i.e. the activity stated as being prohibited has not been carried out"@en ;
    skos:inScheme dpv:rules-classes ;
    skos:prefLabel "Prohibition Unviolated"@en .

dpv:ProhibitionViolated a rdfs:Class,
        skos:Concept,
        dpv:RuleFulfilmentStatus ;
    dct:contributor _:person-harshvardhan-j-pandit ;
    dct:created "2024-09-10"^^xsd:date ;
    rdfs:isDefinedBy dpv: ;
    sw:term_status "accepted"@en ;
    skos:broader dpv:RuleViolated ;
    skos:definition "Status indicating a prohibition has been violated i.e. the activity stated as being prohibited has been carried out"@en ;
    skos:inScheme dpv:rules-classes ;
    skos:prefLabel "Prohibition Violated"@en .

dpv:Recommendation a rdfs:Class,
        skos:Concept,
        dpv:Rule ;
    dct:contributor _:person-arthit-suriyawongkul,
        _:person-beatriz-esteves,
        _:person-delaram-golpayegani,
        _:person-georg-p-krog,
        _:person-harshvardhan-j-pandit,
        _:person-julian-flake,
        _:person-paul-ryan ;
    dct:created "2025-06-19"^^xsd:date ;
    rdfs:isDefinedBy dpv: ;
    sw:term_status "accepted"@en ;
    skos:broader dpv:AcceptableRule ;
    skos:definition "A rule describing a recommendation for performing an activity"@en ;
    skos:inScheme dpv:rules-classes ;
    skos:prefLabel "Recommendation"@en ;
    skos:scopeNote "Recommendations are aligned with the term SHOULD in RFC2119 where specified activities should be carried out but are not obligations"@en .

dpv:RecommendationFollowed a rdfs:Class,
        skos:Concept,
        dpv:RuleFulfilmentStatus ;
    dct:contributor _:person-beatriz-esteves,
        _:person-georg-p-krog,
        _:person-harshvardhan-j-pandit,
        _:person-julian-flake ;
    dct:created "2025-08-06"^^xsd:date ;
    rdfs:isDefinedBy dpv: ;
    sw:term_status "accepted"@en ;
    skos:broader dpv:RuleFulfilled ;
    skos:definition "Status indicating a recommendation has been followed i.e. the activity stated as being recommended has been carried out"@en ;
    skos:inScheme dpv:rules-classes ;
    skos:prefLabel "Recommendation Followed"@en .

dpv:RecommendationNotFollowed a rdfs:Class,
        skos:Concept,
        dpv:RuleFulfilmentStatus ;
    dct:contributor _:person-beatriz-esteves,
        _:person-georg-p-krog,
        _:person-harshvardhan-j-pandit,
        _:person-julian-flake ;
    dct:created "2025-08-06"^^xsd:date ;
    rdfs:isDefinedBy dpv: ;
    sw:term_status "accepted"@en ;
    skos:broader dpv:RuleUnfulfilled ;
    skos:definition "Status indicating a recommendation has not been followed i.e. the activity stated as being recommended has not been carried out"@en ;
    skos:inScheme dpv:rules-classes ;
    skos:prefLabel "Recommendation Not Followed"@en .

dpv:Rule a rdfs:Class,
        skos:Concept ;
    dct:contributor _:person-beatriz-esteves,
        _:person-georg-p-krog,
        _:person-harshvardhan-j-pandit,
        _:person-paul-ryan ;
    dct:created "2022-10-19"^^xsd:date ;
    vann:example dex:E0030 ;
    rdfs:isDefinedBy dpv: ;
    sw:term_status "accepted"@en ;
    skos:definition "A rule describing a process or control that directs or determines if and how an activity should be conducted"@en ;
    skos:inScheme dpv:rules-classes ;
    skos:prefLabel "Rule"@en .

dpv:RuleFulfilled a rdfs:Class,
        skos:Concept,
        dpv:RuleFulfilmentStatus ;
    dct:contributor _:person-harshvardhan-j-pandit ;
    dct:created "2024-09-10"^^xsd:date ;
    rdfs:isDefinedBy dpv: ;
    sw:term_status "accepted"@en ;
    skos:broader dpv:RuleFulfilmentStatus ;
    skos:definition "Status indicating a rule has been fulfilled, completed, or satisfied"@en ;
    skos:inScheme dpv:rules-classes ;
    skos:prefLabel "Rule Fulfilled"@en .

dpv:RuleFulfilmentStatus a rdfs:Class,
        skos:Concept ;
    dct:contributor _:person-harshvardhan-j-pandit ;
    dct:created "2024-09-10"^^xsd:date ;
    vann:example dex:E0084 ;
    rdfs:isDefinedBy dpv: ;
    rdfs:subClassOf dpv:Status ;
    sw:term_status "accepted"@en ;
    skos:broader dpv:Status ;
    skos:definition "Status associated with a rule for indicating whether it is applicable, or has been utilised, and whether the requirements of the rule have been fulfilled or violated"@en ;
    skos:inScheme dpv:rules-classes ;
    skos:prefLabel "Rule Fulfilment Status"@en .

dpv:RuleUnfulfilled a rdfs:Class,
        skos:Concept,
        dpv:RuleFulfilmentStatus ;
    dct:contributor _:person-harshvardhan-j-pandit ;
    dct:created "2024-09-10"^^xsd:date ;
    rdfs:isDefinedBy dpv: ;
    sw:term_status "accepted"@en ;
    skos:broader dpv:RuleFulfilmentStatus ;
    skos:definition "Status indicating a rule has not been fulfilled nor violated"@en ;
    skos:inScheme dpv:rules-classes ;
    skos:prefLabel "Rule Unfulfilled"@en .

dpv:RuleViolated a rdfs:Class,
        skos:Concept,
        dpv:RuleFulfilmentStatus ;
    dct:contributor _:person-harshvardhan-j-pandit ;
    dct:created "2024-09-10"^^xsd:date ;
    rdfs:isDefinedBy dpv: ;
    sw:term_status "accepted"@en ;
    skos:broader dpv:RuleFulfilmentStatus ;
    skos:definition "Status indicating a rule has been violated, breached, broken, or infracted"@en ;
    skos:inScheme dpv:rules-classes ;
    skos:prefLabel "Rule Violated"@en .

dpv:UnacceptableRule a rdfs:Class,
        skos:Concept,
        dpv:Rule ;
    dct:contributor _:person-arthit-suriyawongkul,
        _:person-beatriz-esteves,
        _:person-delaram-golpayegani,
        _:person-georg-p-krog,
        _:person-harshvardhan-j-pandit,
        _:person-julian-flake,
        _:person-paul-ryan ;
    dct:created "2025-06-19"^^xsd:date ;
    rdfs:isDefinedBy dpv: ;
    sw:term_status "accepted"@en ;
    skos:broader dpv:Rule ;
    skos:definition "A rule that is unacceptable where it is not desirable if it occurs"@en ;
    skos:inScheme dpv:rules-classes ;
    skos:prefLabel "Unacceptable Rule"@en ;
    skos:scopeNote "Unacceptable is a subjective concept that enables specifying something is to be avoided as compared to \"acceptable\". By itself it does not signal any deterrence or prohibition - for which further specific concepts are defined"@en .

<https://w3id.org/dpv> a owl:Ontology,
        profile:Profile ;
    dct:bibliographicCitation "Harshvardhan J. Pandit, Beatriz Esteves, Georg P. Krog, Paul Ryan, Delaram Golpayegani, Julian Flake (2025) Data Privacy Vocabulary (DPV) – Version 2.0. In: Demartini, G., et al. The Semantic Web – ISWC 2024. ISWC 2024. Lecture Notes in Computer Science, vol 15233. Springer, Cham. https://doi.org/10.1007/978-3-031-77847-6_10" ;
    dct:conformsTo "http://www.w3.org/2000/01/rdf-schema",
        "http://www.w3.org/2004/02/skos/core" ;
    dct:contributor _:person-arthit-suriyawongkul,
        _:person-beatriz-esteves,
        _:person-delaram-golpayegani,
        _:person-georg-p-krog,
        _:person-harshvardhan-j-pandit,
        _:person-julian-flake,
        _:person-paul-ryan ;
    dct:created "2022-08-18"@en ;
    dct:creator _:person-beatriz-esteves,
        _:person-delaram-golpayegani,
        _:person-georg-p-krog,
        _:person-harshvardhan-j-pandit,
        _:person-julian-flake,
        _:person-paul-ryan ;
    dct:description "The Data Privacy Vocabulary (DPV) provides terms (classes and properties) to represent information about processing of personal data, for example - purposes, processing operations, personal data, technical and organisational measures."@en ;
    dct:identifier "https://w3id.org/dpv" ;
    dct:issued "2022-08-18"@en ;
    dct:license <https://www.w3.org/copyright/document-license-2023/> ;
    dct:modified "2026-02-25"@en ;
    dct:publisher <https://www.w3.org/> ;
    dct:source <https://www.w3.org/groups/cg/dpvcg/> ;
    dct:title "Data Privacy Vocabulary (DPV)"@en ;
    bibo:doi "10.5281/zenodo.12505841" ;
    bibo:status "http://purl.org/ontology/bibo/status/published" ;
    vann:preferredNamespacePrefix "dpv" ;
    vann:preferredNamespaceUri "https://w3id.org/dpv#" ;
    rdfs:Label "DPV"@en ;
    owl:versionIRI <https://w3id.org/dpv/2.3> ;
    owl:versionInfo "2.3" ;
    profile:hasResource dpv:serialisation-html,
        dpv:serialisation-jsonld,
        dpv:serialisation-n3,
        dpv:serialisation-rdf,
        dpv:serialisation-ttl,
        <https://w3id.org/dpv/examples>,
        <https://w3id.org/dpv/guides>,
        <https://w3id.org/dpv/primer> ;
    profile:isProfileOf rdfs:,
        skos: ;
    foaf:logo <https://w3id.org/dpv/media/logo.png> ;
    schema:version "2.3" .

dpv:hasDeterrence a rdf:Property,
        skos:Concept ;
    dcam:domainIncludes dpv:Context ;
    dcam:rangeIncludes dpv:Deterrence ;
    dct:contributor _:person-arthit-suriyawongkul,
        _:person-beatriz-esteves,
        _:person-delaram-golpayegani,
        _:person-georg-p-krog,
        _:person-harshvardhan-j-pandit,
        _:person-julian-flake,
        _:person-paul-ryan ;
    dct:created "2025-06-19"^^xsd:date ;
    rdfs:isDefinedBy dpv: ;
    rdfs:subPropertyOf dpv:hasRule ;
    sw:term_status "accepted"@en ;
    skos:broader dpv:hasRule ;
    skos:definition "Specifies applicability or inclusion of a deterrence rule within specified context"@en ;
    skos:inScheme dpv:rules-properties ;
    skos:prefLabel "has deterrence"@en ;
    schema:domainIncludes dpv:Context ;
    schema:rangeIncludes dpv:Deterrence .

dpv:hasFulfilmentStatus a rdf:Property,
        skos:Concept ;
    dcam:domainIncludes dpv:Context ;
    dcam:rangeIncludes dpv:Rule ;
    dct:contributor _:person-harshvardhan-j-pandit ;
    dct:created "2024-09-10"^^xsd:date ;
    dct:modified "2025-06-19"^^xsd:date ;
    rdfs:isDefinedBy dpv: ;
    rdfs:subPropertyOf dpv:hasStatus ;
    sw:term_status "modified"@en ;
    skos:broader dpv:hasStatus ;
    skos:definition "Specifies the fulfillment status associated with a rule"@en ;
    skos:inScheme dpv:rules-properties ;
    skos:prefLabel "has fulfilment status"@en ;
    schema:domainIncludes dpv:Context ;
    schema:rangeIncludes dpv:Rule .

dpv:hasObligation a rdf:Property,
        skos:Concept ;
    dcam:domainIncludes dpv:Context ;
    dcam:rangeIncludes dpv:Obligation ;
    dct:contributor _:person-beatriz-esteves,
        _:person-georg-p-krog,
        _:person-harshvardhan-j-pandit,
        _:person-paul-ryan ;
    dct:created "2022-10-19"^^xsd:date ;
    rdfs:isDefinedBy dpv: ;
    rdfs:subPropertyOf dpv:hasRule ;
    sw:term_status "accepted"@en ;
    skos:broader dpv:hasRule ;
    skos:definition "Specifies applicability or inclusion of an obligation rule within specified context"@en ;
    skos:inScheme dpv:rules-properties ;
    skos:prefLabel "has obligation"@en ;
    schema:domainIncludes dpv:Context ;
    schema:rangeIncludes dpv:Obligation .

dpv:hasPermission a rdf:Property,
        skos:Concept ;
    dcam:domainIncludes dpv:Context ;
    dcam:rangeIncludes dpv:Permission ;
    dct:contributor _:person-beatriz-esteves,
        _:person-georg-p-krog,
        _:person-harshvardhan-j-pandit,
        _:person-paul-ryan ;
    dct:created "2022-10-19"^^xsd:date ;
    vann:example dex:E0066 ;
    rdfs:isDefinedBy dpv: ;
    rdfs:subPropertyOf dpv:hasRule ;
    sw:term_status "accepted"@en ;
    skos:broader dpv:hasRule ;
    skos:definition "Specifies applicability or inclusion of a permission rule within specified context"@en ;
    skos:inScheme dpv:rules-properties ;
    skos:prefLabel "has permission"@en ;
    schema:domainIncludes dpv:Context ;
    schema:rangeIncludes dpv:Permission .

dpv:hasProhibition a rdf:Property,
        skos:Concept ;
    dcam:domainIncludes dpv:Context ;
    dcam:rangeIncludes dpv:Prohibition ;
    dct:contributor _:person-beatriz-esteves,
        _:person-georg-p-krog,
        _:person-harshvardhan-j-pandit,
        _:person-paul-ryan ;
    dct:created "2022-10-19"^^xsd:date ;
    vann:example dex:E0066 ;
    rdfs:isDefinedBy dpv: ;
    rdfs:subPropertyOf dpv:hasRule ;
    sw:term_status "accepted"@en ;
    skos:broader dpv:hasRule ;
    skos:definition "Specifies applicability or inclusion of a prohibition rule within specified context"@en ;
    skos:inScheme dpv:rules-properties ;
    skos:prefLabel "has prohibition"@en ;
    schema:domainIncludes dpv:Context ;
    schema:rangeIncludes dpv:Prohibition .

dpv:hasRecommendation a rdf:Property,
        skos:Concept ;
    dcam:domainIncludes dpv:Context ;
    dcam:rangeIncludes dpv:Recommendation ;
    dct:contributor _:person-arthit-suriyawongkul,
        _:person-beatriz-esteves,
        _:person-delaram-golpayegani,
        _:person-georg-p-krog,
        _:person-harshvardhan-j-pandit,
        _:person-julian-flake,
        _:person-paul-ryan ;
    dct:created "2025-06-19"^^xsd:date ;
    rdfs:isDefinedBy dpv: ;
    rdfs:subPropertyOf dpv:hasRule ;
    sw:term_status "accepted"@en ;
    skos:broader dpv:hasRule ;
    skos:definition "Specifies applicability or inclusion of a recommendation rule within specified context"@en ;
    skos:inScheme dpv:rules-properties ;
    skos:prefLabel "has recommendation"@en ;
    schema:domainIncludes dpv:Context ;
    schema:rangeIncludes dpv:Recommendation .

dpv:serialisation-html a profile:ResourceDescriptor ;
    dct:conformsTo <https://www.w3.org/TR/html/> ;
    dct:format <https://www.iana.org/assignments/media-types/text/html> ;
    dct:title "Data Privacy Vocabulary (DPV) - HTML serialisation" ;
    profile:hasArtifact <https://w3id.org/dpv/dpv.html> ;
    profile:hasRole role:specification .

dpv:serialisation-jsonld a profile:ResourceDescriptor ;
    dct:conformsTo <https://www.w3.org/TR/json-ld11/> ;
    dct:format <https://www.iana.org/assignments/media-types/application/ld+json> ;
    dct:title "Data Privacy Vocabulary (DPV) - JSON-LD serialisation" ;
    profile:hasArtifact <https://w3id.org/dpv/dpv/dpv.jsonld> ;
    profile:hasRole role:vocabulary .

dpv:serialisation-n3 a profile:ResourceDescriptor ;
    dct:conformsTo <https://www.w3.org/TeamSubmission/n3/> ;
    dct:format <https://www.iana.org/assignments/media-types/text/n3> ;
    dct:title "Data Privacy Vocabulary (DPV) - N3 serialisation" ;
    profile:hasArtifact <https://w3id.org/dpv/dpv/dpv.n3> ;
    profile:hasRole role:vocabulary .

dpv:serialisation-rdf a profile:ResourceDescriptor ;
    dct:conformsTo rdf: ;
    dct:format <https://www.iana.org/assignments/media-types/application/rdf+xml> ;
    dct:title "Data Privacy Vocabulary (DPV) - RDF/XML serialisation" ;
    profile:hasArtifact <https://w3id.org/dpv/dpv/dpv.rdf> ;
    profile:hasRole role:vocabulary .

dpv:serialisation-ttl a profile:ResourceDescriptor ;
    dct:conformsTo <https://www.w3.org/TR/turtle/> ;
    dct:format <https://www.iana.org/assignments/media-types/text/turtle> ;
    dct:title "Data Privacy Vocabulary (DPV) - Turtle serialisation" ;
    profile:hasArtifact <https://w3id.org/dpv/dpv/dpv.ttl> ;
    profile:hasRole role:vocabulary .

<https://w3id.org/dpv/examples> a profile:ResourceDescriptor ;
    dct:conformsTo <https://www.w3.org/TR/html/> ;
    dct:format <https://www.iana.org/assignments/media-types/text/html> ;
    dct:title "Examples" ;
    profile:hasArtifact <https://w3id.org/dpv/examples> ;
    profile:hasRole role:guidance .

<https://w3id.org/dpv/guides> a profile:ResourceDescriptor ;
    dct:conformsTo <https://www.w3.org/TR/html/> ;
    dct:format <https://www.iana.org/assignments/media-types/text/html> ;
    dct:title "Guides for Data Privacy Vocabulary" ;
    profile:hasArtifact <https://w3id.org/dpv/guides> ;
    profile:hasRole role:guidance .

<https://w3id.org/dpv/primer> a profile:ResourceDescriptor ;
    dct:conformsTo <https://www.w3.org/TR/html/> ;
    dct:format <https://www.iana.org/assignments/media-types/text/html> ;
    dct:title "Primer for Data Privacy Vocabulary" ;
    profile:hasArtifact <https://w3id.org/dpv/primer> ;
    profile:hasRole role:guidance .

dpv:rules-properties a skos:ConceptScheme .

dpv:hasRule a rdf:Property,
        skos:Concept ;
    dcam:domainIncludes dpv:Context ;
    dcam:rangeIncludes dpv:Rule ;
    dct:contributor _:person-beatriz-esteves,
        _:person-georg-p-krog,
        _:person-harshvardhan-j-pandit,
        _:person-paul-ryan ;
    dct:created "2022-10-19"^^xsd:date ;
    rdfs:isDefinedBy dpv: ;
    sw:term_status "accepted"@en ;
    skos:definition "Specifies applicability or inclusion of a rule within specified context"@en ;
    skos:inScheme dpv:rules-properties ;
    skos:prefLabel "has rule"@en ;
    schema:domainIncludes dpv:Context ;
    schema:rangeIncludes dpv:Rule .

dpv:rules-classes a skos:ConceptScheme .

_:org-ai-accountability-lab-aial-trinity-college-dublin a foaf:Organization ;
    foaf:name "AI Accountability Lab (AIAL), Trinity College Dublin" .

_:org-idlab-imec-ghent-university a foaf:Organization ;
    foaf:name "IDLab, IMEC, Ghent University" .

_:org-signatu-as a foaf:Organization ;
    foaf:name "Signatu AS" .

_:org-uniphar-plc a foaf:Organization ;
    foaf:name "Uniphar PLC" .

_:org-university-of-koblenz a foaf:Organization ;
    foaf:name "University of Koblenz" .

_:org-adapt-centre-trinity-college-dublin a foaf:Organization ;
    foaf:name "ADAPT Centre, Trinity College Dublin" .

_:person-arthit-suriyawongkul a dct:Agent,
        foaf:Person ;
    scoro:hasORCID "0000-0002-9698-1899" ;
    org:memberOf _:org-adapt-centre-trinity-college-dublin ;
    foaf:name "Arthit Suriyawongkul" .

_:person-delaram-golpayegani a dct:Agent,
        foaf:Person ;
    scoro:hasORCID "0000-0002-1208-186X" ;
    org:memberOf _:org-adapt-centre-trinity-college-dublin ;
    foaf:name "Delaram Golpayegani" .

_:person-julian-flake a dct:Agent,
        foaf:Person ;
    scoro:hasORCID "0009-0006-4623-1463" ;
    org:memberOf _:org-university-of-koblenz ;
    foaf:name "Julian Flake" .

_:person-paul-ryan a dct:Agent,
        foaf:Person ;
    scoro:hasORCID "0000-0003-0770-2737" ;
    org:memberOf _:org-uniphar-plc ;
    foaf:name "Paul Ryan" .

_:person-beatriz-esteves a dct:Agent,
        foaf:Person ;
    scoro:hasORCID "0000-0003-0259-7560" ;
    org:memberOf _:org-idlab-imec-ghent-university ;
    foaf:homepage "https://w3id.org/people/besteves" ;
    foaf:name "Beatriz Esteves" .

_:person-georg-p-krog a dct:Agent,
        foaf:Person ;
    org:memberOf _:org-signatu-as ;
    foaf:homepage "https://www.linkedin.com/in/georg-philip-krog-a2a278104/" ;
    foaf:name "Georg P. Krog" .

_:person-harshvardhan-j-pandit a dct:Agent,
        foaf:Person ;
    scoro:hasORCID "0000-0002-5068-3714" ;
    org:memberOf _:org-ai-accountability-lab-aial-trinity-college-dublin ;
    foaf:homepage "https://harshp.com/" ;
    foaf:name "Harshvardhan J. Pandit" .

