@prefix bibo: <http://purl.org/ontology/bibo/> .
@prefix dcam: <http://purl.org/dc/dcam/> .
@prefix dct: <http://purl.org/dc/terms/> .
@prefix dex-owl: <https://w3id.org/dpv/examples/owl#> .
@prefix dpv-owl: <https://w3id.org/dpv/owl#> .
@prefix foaf: <http://xmlns.com/foaf/0.1/> .
@prefix owl: <http://www.w3.org/2002/07/owl#> .
@prefix profile: <http://www.w3.org/ns/dx/prof/> .
@prefix rdf: <http://www.w3.org/1999/02/22-rdf-syntax-ns#> .
@prefix rdfs: <http://www.w3.org/2000/01/rdf-schema#> .
@prefix role: <http://www.w3.org/ns/dx/prof/role/> .
@prefix schema: <https://schema.org/> .
@prefix skos: <http://www.w3.org/2004/02/skos/core#> .
@prefix sw: <http://www.w3.org/2003/06/sw-vocab-status/ns#> .
@prefix tech-owl: <https://w3id.org/dpv/tech/owl#> .
@prefix vann: <http://purl.org/vocab/vann/> .
@prefix xsd: <http://www.w3.org/2001/XMLSchema#> .

tech-owl:Actor a rdfs:Class,
        owl:Class ;
    dct:contributor "Harshvardhan J. Pandit, Delaram Golpayegani" ;
    dct:created "2022-06-15"^^xsd:date ;
    rdfs:isDefinedBy tech-owl: ;
    rdfs:subClassOf dpv-owl:Entity ;
    sw:term_status "accepted"@en ;
    skos:definition "Actors and Entities involved in provision, use, and management of Technology"@en ;
    skos:prefLabel "Actor"@en .

tech-owl:Capability a rdfs:Class,
        owl:Class ;
    dct:created "2024-05-09"^^xsd:date ;
    vann:example dex-owl:E0064 ;
    rdfs:isDefinedBy tech-owl: ;
    rdfs:subClassOf rdfs:Class ;
    sw:term_status "accepted"@en ;
    skos:definition "Expression of what the technology is capable of achieving or providing"@en ;
    skos:prefLabel "Capability"@en ;
    skos:scopeNote "Examples of capabilities are image recognition, sentiment analysis, machine translation"@en .

tech-owl:CommunicationMechanism a rdfs:Class,
        owl:Class ;
    dct:contributor "Harshvardhan J. Pandit" ;
    dct:created "2022-06-15"^^xsd:date ;
    rdfs:isDefinedBy tech-owl: ;
    rdfs:subClassOf dpv-owl:Technology ;
    sw:term_status "accepted"@en ;
    skos:definition "Communication mechanism used or provided by Technology"@en ;
    skos:prefLabel "Communication Mechanism"@en .

tech-owl:DeploymentLocation a rdfs:Class,
        owl:Class ;
    dct:contributor "Harshvardhan J. Pandit, Delaram Golpayegani" ;
    dct:created "2022-06-15"^^xsd:date ;
    rdfs:isDefinedBy tech-owl: ;
    rdfs:subClassOf dpv-owl:Location ;
    sw:term_status "accepted"@en ;
    skos:definition "Location for where technology is deployed and used"@en ;
    skos:prefLabel "Deployment Location"@en .

tech-owl:Documentation a rdfs:Class,
        owl:Class ;
    dct:created "2024-05-09"^^xsd:date ;
    rdfs:isDefinedBy tech-owl: ;
    rdfs:subClassOf rdfs:Class ;
    sw:term_status "accepted"@en ;
    skos:definition "Information describing use, functionality, design, or other technical aspects of the Technology"@en ;
    skos:prefLabel "Documentation"@en .

tech-owl:Function a rdfs:Class,
        owl:Class ;
    dct:created "2024-05-09"^^xsd:date ;
    rdfs:isDefinedBy tech-owl: ;
    rdfs:subClassOf rdfs:Class ;
    sw:term_status "accepted"@en ;
    skos:definition "Expression of what goals or purposes the technology's capabilities are being used towards or developed for"@en ;
    skos:prefLabel "Function"@en ;
    skos:scopeNote "Function is a broad concept that can include purposes such as identify verification, capability such as image recognition, or specific security measures such as encryption"@en .

tech-owl:IntendedUse a rdfs:Class,
        owl:Class ;
    dct:contributor "Harshvardhan J. Pandit" ;
    dct:created "2024-05-22"^^xsd:date ;
    rdfs:isDefinedBy tech-owl: ;
    rdfs:subClassOf rdfs:Class ;
    sw:term_status "accepted"@en ;
    skos:definition "Describes the 'intended' use of the technology"@en ;
    skos:prefLabel "Intended Use"@en ;
    skos:scopeNote "Intended use can be used to describe how the developer or provider of technology intends it to be used e.g. use a database to store data, and to describe the plan or 'intent' to use the technology by a user or operator e.g. use a database to store and analyse data. Intended Use can involve any concept e.g. DPV's purpose, processing, tech/org measures, and can be low-level purely technical uses such as store data or high-level goals such as legal compliance. Intended Use only describes the intent or ex-ante intention, and may be different from how the technology is being actually used - which is indicated by using isImplementedUsingTechnology in a process or other relevant context."@en .

tech-owl:ProvisionMethod a rdfs:Class,
        owl:Class ;
    dct:contributor "Harshvardhan J. Pandit, Delaram Golpayegani" ;
    dct:created "2022-06-15"^^xsd:date ;
    dct:modified "2024-05-09"^^xsd:date ;
    rdfs:isDefinedBy tech-owl: ;
    rdfs:subClassOf dpv-owl:Technology ;
    sw:term_status "accepted"@en ;
    skos:definition "Method associated with provision or use of technology"@en ;
    skos:prefLabel "Provision Method"@en .

tech-owl:hasActor a rdf:Property,
        owl:ObjectProperty ;
    dcam:domainIncludes dpv-owl:Technology ;
    dcam:rangeIncludes tech-owl:TechnologyActor ;
    dct:contributor "Harshvardhan J. Pandit" ;
    dct:created "2022-10-21"^^xsd:date ;
    dct:modified "2024-05-17"^^xsd:date ;
    rdfs:isDefinedBy tech-owl: ;
    sw:term_status "accepted"@en ;
    skos:definition "Indicates an actor associated with technology"@en ;
    skos:prefLabel "has actor"@en ;
    schema:domainIncludes dpv-owl:Technology ;
    schema:rangeIncludes tech-owl:TechnologyActor .

tech-owl:hasCapability a rdf:Property,
        owl:ObjectProperty ;
    dcam:domainIncludes dpv-owl:Technology ;
    dcam:rangeIncludes tech-owl:Capability ;
    dct:created "2024-05-09"^^xsd:date ;
    vann:example dex-owl:E0064 ;
    rdfs:isDefinedBy tech-owl: ;
    sw:term_status "accepted"@en ;
    skos:definition "Indicates the capability of the technology"@en ;
    skos:prefLabel "has capability"@en ;
    schema:domainIncludes dpv-owl:Technology ;
    schema:rangeIncludes tech-owl:Capability .

tech-owl:hasCommunicationMechanism a rdf:Property,
        owl:ObjectProperty ;
    dcam:domainIncludes dpv-owl:Technology ;
    dcam:rangeIncludes tech-owl:CommunicationMechanism ;
    dct:contributor "Harshvardhan J. Pandit" ;
    dct:created "2022-07-02"^^xsd:date ;
    rdfs:isDefinedBy tech-owl: ;
    sw:term_status "accepted"@en ;
    skos:definition "Indicates communication mechanisms used or provided by technology"@en ;
    skos:prefLabel "has communication mechanism"@en ;
    schema:domainIncludes dpv-owl:Technology ;
    schema:rangeIncludes tech-owl:CommunicationMechanism .

tech-owl:hasDeploymentLocation a rdf:Property,
        owl:ObjectProperty ;
    dcam:domainIncludes dpv-owl:Technology ;
    dcam:rangeIncludes tech-owl:DeploymentLocation ;
    dct:contributor "Harshvardhan J. Pandit" ;
    dct:created "2024-05-09"^^xsd:date ;
    rdfs:isDefinedBy tech-owl: ;
    sw:term_status "accepted"@en ;
    skos:definition "Specifies the location of technology deployment and use"@en ;
    skos:prefLabel "has deployment location"@en ;
    schema:domainIncludes dpv-owl:Technology ;
    schema:rangeIncludes tech-owl:DeploymentLocation .

tech-owl:hasDocumentation a rdf:Property,
        owl:ObjectProperty ;
    dcam:domainIncludes dpv-owl:Technology ;
    dcam:rangeIncludes tech-owl:Documentation ;
    dct:contributor "Harshvardhan J. Pandit" ;
    dct:created "2024-06-29"^^xsd:date ;
    rdfs:isDefinedBy tech-owl: ;
    sw:term_status "accepted"@en ;
    skos:definition "Indicates documentation associated with technology"@en ;
    skos:prefLabel "has documentation"@en ;
    schema:domainIncludes dpv-owl:Technology ;
    schema:rangeIncludes tech-owl:Documentation .

tech-owl:hasFunction a rdf:Property,
        owl:ObjectProperty ;
    dcam:domainIncludes dpv-owl:Technology ;
    dcam:rangeIncludes tech-owl:Function ;
    dct:created "2024-05-09"^^xsd:date ;
    rdfs:isDefinedBy tech-owl: ;
    sw:term_status "accepted"@en ;
    skos:definition "Indicates the function of the technology"@en ;
    skos:prefLabel "has function"@en ;
    schema:domainIncludes dpv-owl:Technology ;
    schema:rangeIncludes tech-owl:Function .

tech-owl:hasIntendedUse a rdf:Property,
        owl:ObjectProperty ;
    dcam:domainIncludes dpv-owl:Technology ;
    dcam:rangeIncludes tech-owl:IntendedUse ;
    dct:contributor "Harshvardhan J. Pandit" ;
    dct:created "2024-05-22"^^xsd:date ;
    rdfs:isDefinedBy tech-owl: ;
    sw:term_status "accepted"@en ;
    skos:definition "Indicates the intended use of technology"@en ;
    skos:prefLabel "has intended use"@en ;
    schema:domainIncludes dpv-owl:Technology ;
    schema:rangeIncludes tech-owl:IntendedUse .

tech-owl:hasProvisionMethod a rdf:Property,
        owl:ObjectProperty ;
    dcam:domainIncludes dpv-owl:Technology ;
    dcam:rangeIncludes tech-owl:ProvisionMethod ;
    dct:contributor "Harshvardhan J. Pandit" ;
    dct:created "2022-07-02"^^xsd:date ;
    rdfs:isDefinedBy tech-owl: ;
    sw:term_status "accepted"@en ;
    skos:definition "Specifies the provision or usage method of technology"@en ;
    skos:prefLabel "has provision method"@en ;
    schema:domainIncludes dpv-owl:Technology ;
    schema:rangeIncludes tech-owl:ProvisionMethod .

tech-owl:serialisation-html a profile:ResourceDescriptor ;
    dct:conformsTo <https://www.w3.org/TR/html/> ;
    dct:format <https://www.iana.org/assignments/media-types/text/html> ;
    dct:title "Technology Concepts - HTML serialiation" ;
    profile:hasArtifact <https://w3id.org/dpv/tech/tech-owl.html> ;
    profile:hasRole role:specification .

tech-owl:serialisation-jsonld a profile:ResourceDescriptor ;
    dct:conformsTo <https://www.w3.org/TR/json-ld11/> ;
    dct:format <https://www.iana.org/assignments/media-types/application/ld+json> ;
    dct:title "Technology Concepts - JSON-LD serialiation" ;
    profile:hasArtifact <https://w3id.org/dpv/tech/tech-owl.jsonld> ;
    profile:hasRole role:vocabulary .

tech-owl:serialisation-n3 a profile:ResourceDescriptor ;
    dct:conformsTo <https://www.w3.org/TeamSubmission/n3/> ;
    dct:format <https://www.iana.org/assignments/media-types/text/n3> ;
    dct:title "Technology Concepts - N3 serialiation" ;
    profile:hasArtifact <https://w3id.org/dpv/tech/tech-owl.n3> ;
    profile:hasRole role:vocabulary .

tech-owl:serialisation-rdf a profile:ResourceDescriptor ;
    dct:conformsTo rdf: ;
    dct:format <https://www.iana.org/assignments/media-types/application/rdf+xml> ;
    dct:title "Technology Concepts - RDF/XML serialiation" ;
    profile:hasArtifact <https://w3id.org/dpv/tech/tech-owl.rdf> ;
    profile:hasRole role:vocabulary .

tech-owl:serialisation-ttl a profile:ResourceDescriptor ;
    dct:conformsTo <https://www.w3.org/TR/turtle/> ;
    dct:format <https://www.iana.org/assignments/media-types/text/turtle> ;
    dct:title "Technology Concepts - Turtle serialiation" ;
    profile:hasArtifact <https://w3id.org/dpv/tech/tech-owl.ttl> ;
    profile:hasRole role:vocabulary .

<https://w3id.org/dpv/examples> a profile:ResourceDescriptor ;
    dct:conformsTo <https://www.w3.org/TR/html/> ;
    dct:format <https://www.iana.org/assignments/media-types/text/html> ;
    dct:title "Examples for Data Privacy Vocabulary" ;
    profile:hasArtifact <https://w3id.org/dpv/examples> ;
    profile:hasRole role:guidance .

<https://w3id.org/dpv/guides> a profile:ResourceDescriptor ;
    dct:conformsTo <https://www.w3.org/TR/html/> ;
    dct:format <https://www.iana.org/assignments/media-types/text/html> ;
    dct:title "Guides for Data Privacy Vocabulary" ;
    profile:hasArtifact <https://w3id.org/dpv/guides> ;
    profile:hasRole role:guidance .

<https://w3id.org/dpv/primer> a profile:ResourceDescriptor ;
    dct:conformsTo <https://www.w3.org/TR/html/> ;
    dct:format <https://www.iana.org/assignments/media-types/text/html> ;
    dct:title "Primer for Data Privacy Vocabulary" ;
    profile:hasArtifact <https://w3id.org/dpv/primer> ;
    profile:hasRole role:guidance .

tech-owl: a owl:Ontology,
        profile:Profile ;
    dct:bibliographicCitation "Data Privacy Vocabulary (DPV) -- Version 2. Harshvardhan J. Pandit, Beatriz Esteves, Georg P. Krog, Paul Ryan, Delaram Golpayegani, Julian Flake https://doi.org/10.48550/arXiv.2404.13426" ;
    dct:conformsTo <http://www.w3.org/2002/07/owl>,
        "http://www.w3.org/2000/01/rdf-schema",
        "http://www.w3.org/2004/02/skos/core" ;
    dct:contributor "Delaram Golpayegani",
        "Harshvardhan J. Pandit" ;
    dct:created "2024-05-31"@en ;
    dct:creator "Delaram Golpayegani"@en,
        "Georg P Krog"@en,
        "Harshvardhan J. Pandit"@en,
        "Julian Flake"@en,
        "Paul Ryan"@en ;
    dct:description "Extension to the Data Privacy Vocabulary (DPV) providing concepts for representing information about technologies and its provision"@en ;
    dct:hasVersion tech-owl: ;
    dct:identifier "https://w3id.org/dpv/tech" ;
    dct:issued "2024-05-31"@en ;
    dct:license <https://www.w3.org/copyright/document-license-2023/> ;
    dct:modified "2024-07-01"@en ;
    dct:publisher <https://www.w3.org/> ;
    dct:source <https://www.w3.org/groups/cg/dpvcg/> ;
    dct:title "Technology Concepts"@en ;
    bibo:doi "10.5281/zenodo.12505841" ;
    bibo:status "http://purl.org/ontology/bibo/status/published" ;
    vann:preferredNamespacePrefix "tech" ;
    vann:preferredNamespaceUri "https://w3id.org/dpv/tech#" ;
    rdfs:Label "TECH"@en ;
    owl:versionIRI <https://w3id.org/dpv/2.0/tech/owl#> ;
    owl:versionInfo "2.0" ;
    profile:hasResource <https://w3id.org/dpv/examples>,
        <https://w3id.org/dpv/guides>,
        <https://w3id.org/dpv/primer>,
        tech-owl:serialisation-html,
        tech-owl:serialisation-jsonld,
        tech-owl:serialisation-n3,
        tech-owl:serialisation-rdf,
        tech-owl:serialisation-ttl ;
    profile:isProfileOf <http://www.w3.org/2002/07/owl>,
        <https://w3id.org/dpv/owl>,
        tech-owl: ;
    foaf:logo <https://w3id.org/dpv/media/logo.png> ;
    schema:version "2.0" .

