@prefix bibo: <http://purl.org/ontology/bibo/> .
@prefix dcam: <http://purl.org/dc/dcam/> .
@prefix dct: <http://purl.org/dc/terms/> .
@prefix dpv: <https://w3id.org/dpv#> .
@prefix foaf: <http://xmlns.com/foaf/0.1/> .
@prefix org: <http://www.w3.org/ns/org#> .
@prefix owl: <http://www.w3.org/2002/07/owl#> .
@prefix p7012: <https://w3id.org/dpv/standards/p7012#> .
@prefix profile: <http://www.w3.org/ns/dx/prof/> .
@prefix rdf: <http://www.w3.org/1999/02/22-rdf-syntax-ns#> .
@prefix rdfs: <http://www.w3.org/2000/01/rdf-schema#> .
@prefix role: <http://www.w3.org/ns/dx/prof/role/> .
@prefix schema: <https://schema.org/> .
@prefix scoro: <http://purl.org/spar/scoro/> .
@prefix skos: <http://www.w3.org/2004/02/skos/core#> .
@prefix sw: <http://www.w3.org/2003/06/sw-vocab-status/ns#> .
@prefix vann: <http://purl.org/vocab/vann/> .
@prefix xsd: <http://www.w3.org/2001/XMLSchema#> .

p7012:Agent a rdfs:Class,
        skos:Concept ;
    dct:created "2024-12-17"^^xsd:date ;
    rdfs:isDefinedBy p7012: ;
    rdfs:subClassOf dpv:Entity ;
    sw:term_status "accepted"@en ;
    skos:broader dpv:Entity ;
    skos:definition "An Agent is any software or a combination of software and hardware that works exclusively for its party, and which may be provided by a third party but must be controlled and be responsible to the party it represents"@en ;
    skos:inScheme p7012:entities-classes ;
    skos:prefLabel "Agent"@en .

p7012:AgentAllowsNegotiation a rdfs:Class,
        skos:Concept,
        p7012:AgentNegotiationBehaviour ;
    dct:created "2024-12-17"^^xsd:date ;
    rdfs:isDefinedBy p7012: ;
    sw:term_status "accepted"@en ;
    skos:broader p7012:AgentNegotiationBehaviour ;
    skos:definition "Term that indicates the Agent should allow negotiations"@en ;
    skos:inScheme p7012:privacy-term-classes ;
    skos:prefLabel "Agent Allows Negotiation"@en .

p7012:AgentAllowsNegotiationOnlyKnownParty a rdfs:Class,
        skos:Concept,
        p7012:AgentNegotiationBehaviour ;
    dct:created "2024-12-17"^^xsd:date ;
    rdfs:isDefinedBy p7012: ;
    sw:term_status "accepted"@en ;
    skos:broader p7012:AgentAllowsNegotiation ;
    skos:definition "Term that indicates the Agent should allow negotiations but only from known parties"@en ;
    skos:inScheme p7012:privacy-term-classes ;
    skos:prefLabel "Agent Allows Negotiation Only Known Party"@en .

p7012:AgentAllowsNegotiationOnlyPriorAgreementParty a rdfs:Class,
        skos:Concept,
        p7012:AgentNegotiationBehaviour ;
    dct:created "2024-12-17"^^xsd:date ;
    rdfs:isDefinedBy p7012: ;
    sw:term_status "accepted"@en ;
    skos:broader p7012:AgentAllowsNegotiationOnlyKnownParty ;
    skos:definition "Term that indicates the Agent should allow negotiations but only from known parties with whom an agreement was established in the past"@en ;
    skos:inScheme p7012:privacy-term-classes ;
    skos:prefLabel "Agent Allows Negotiation Only Prior Agreement Party"@en .

p7012:AgentAllowsRequests a rdfs:Class,
        skos:Concept,
        p7012:AgentRequestBehaviour ;
    dct:created "2024-12-17"^^xsd:date ;
    rdfs:isDefinedBy p7012: ;
    sw:term_status "accepted"@en ;
    skos:broader p7012:AgentRequestBehaviour ;
    skos:definition "Term that indicates the Agent should allow requests to be made"@en ;
    skos:inScheme p7012:privacy-term-classes ;
    skos:prefLabel "Agent Allows Requests"@en .

p7012:AgentAllowsRequestsOnlyKnownParty a rdfs:Class,
        skos:Concept,
        p7012:AgentRequestBehaviour ;
    dct:created "2024-12-17"^^xsd:date ;
    rdfs:isDefinedBy p7012: ;
    sw:term_status "accepted"@en ;
    skos:broader p7012:AgentAllowsRequests ;
    skos:definition "Term that indicates the Agent should allow requests to be made but only from prior known parties"@en ;
    skos:inScheme p7012:privacy-term-classes ;
    skos:prefLabel "Agent Allows Requests Only Known Party"@en .

p7012:AgentAllowsRequestsOnlyPriorAgreementParty a rdfs:Class,
        skos:Concept,
        p7012:AgentRequestBehaviour ;
    dct:created "2024-12-17"^^xsd:date ;
    rdfs:isDefinedBy p7012: ;
    sw:term_status "accepted"@en ;
    skos:broader p7012:AgentAllowsRequestsOnlyKnownParty ;
    skos:definition "Term that indicates the Agent should allow requests to be made but only from prior known parties with whom an agreement was established in the past"@en ;
    skos:inScheme p7012:privacy-term-classes ;
    skos:prefLabel "Agent Allows Requests Only Prior Agreement Party"@en .

p7012:AgentBehaviour a rdfs:Class,
        skos:Concept ;
    dct:created "2024-12-17"^^xsd:date ;
    rdfs:isDefinedBy p7012: ;
    rdfs:subClassOf dpv:ContractualClause ;
    sw:term_status "accepted"@en ;
    skos:broader dpv:ContractualClause ;
    skos:definition "Term that indicates the behaviour of the Agent"@en ;
    skos:inScheme p7012:privacy-term-classes ;
    skos:prefLabel "Agent Behaviour"@en .

p7012:AgentDisallowsNegotiation a rdfs:Class,
        skos:Concept,
        p7012:AgentNegotiationBehaviour ;
    dct:created "2024-12-17"^^xsd:date ;
    rdfs:isDefinedBy p7012: ;
    sw:term_status "accepted"@en ;
    skos:broader p7012:AgentNegotiationBehaviour ;
    skos:definition "Term that indicates the Agent should not allow any negotiations"@en ;
    skos:inScheme p7012:privacy-term-classes ;
    skos:prefLabel "Agent Disallows Negotiation"@en .

p7012:AgentDisallowsRequests a rdfs:Class,
        skos:Concept,
        p7012:AgentRequestBehaviour ;
    dct:created "2024-12-17"^^xsd:date ;
    rdfs:isDefinedBy p7012: ;
    sw:term_status "accepted"@en ;
    skos:broader p7012:AgentRequestBehaviour ;
    skos:definition "Term that indicates the Agent should not allow any requests to be made"@en ;
    skos:inScheme p7012:privacy-term-classes ;
    skos:prefLabel "Agent Disallows Requests"@en .

p7012:AgentNegotiationBehaviour a rdfs:Class,
        skos:Concept ;
    dct:created "2024-12-17"^^xsd:date ;
    rdfs:isDefinedBy p7012: ;
    rdfs:subClassOf p7012:AgentBehaviour ;
    sw:term_status "accepted"@en ;
    skos:broader p7012:AgentBehaviour ;
    skos:definition "Term that indicates the behaviour of the Agent in relation to negotiations"@en ;
    skos:inScheme p7012:privacy-term-classes ;
    skos:prefLabel "Agent Negotiation Behaviour"@en .

p7012:AgentRequestBehaviour a rdfs:Class,
        skos:Concept ;
    dct:created "2024-12-17"^^xsd:date ;
    rdfs:isDefinedBy p7012: ;
    rdfs:subClassOf p7012:AgentBehaviour ;
    sw:term_status "accepted"@en ;
    skos:broader p7012:AgentBehaviour ;
    skos:definition "Term that indicates the behaviour of the Agent in relation to requests"@en ;
    skos:inScheme p7012:privacy-term-classes ;
    skos:prefLabel "Agent Request Behaviour"@en .

p7012:Agreement a rdfs:Class,
        skos:Concept ;
    dct:created "2024-12-17"^^xsd:date ;
    rdfs:isDefinedBy p7012: ;
    rdfs:subClassOf dpv:ContractualClause ;
    sw:term_status "accepted"@en ;
    skos:broader dpv:ContractualClause ;
    skos:definition "A compound set of terms or clauses, proposed and offered before a formal contract between parties, and also referred to as a \"proposal\" pr \"proposed agreement\""@en ;
    skos:inScheme p7012:process-classes ;
    skos:prefLabel "Agreement"@en .

p7012:AgreementAccepted a rdfs:Class,
        skos:Concept,
        p7012:AgreementNegotiationStatus ;
    dct:created "2024-12-17"^^xsd:date ;
    rdfs:isDefinedBy p7012: ;
    sw:term_status "accepted"@en ;
    skos:broader p7012:AgreementNegotiationStatus ;
    skos:definition "Status indicating the Agreement Negotiation is completed and the parties have accepted the relevant terms"@en ;
    skos:inScheme p7012:status-classes ;
    skos:prefLabel "Agreement Accepted"@en .

p7012:AgreementInteractionRecord a rdfs:Class,
        skos:Concept ;
    dct:created "2024-12-17"^^xsd:date ;
    rdfs:isDefinedBy p7012: ;
    rdfs:subClassOf dpv:RecordsOfActivities ;
    sw:term_status "accepted"@en ;
    skos:broader dpv:RecordsOfActivities ;
    skos:definition "A record of a interactions conducted in the course of establishing and negotiating agreements, including failed attemps, creation of contracts, and subsequent interactions"@en ;
    skos:inScheme p7012:process-classes ;
    skos:prefLabel "Agreement Interaction Record"@en .

p7012:AgreementNegotiation a rdfs:Class,
        skos:Concept ;
    dct:created "2024-12-17"^^xsd:date ;
    rdfs:isDefinedBy p7012: ;
    rdfs:subClassOf dpv:Process ;
    sw:term_status "accepted"@en ;
    skos:broader dpv:Process ;
    skos:definition "A negotiation between parties regarding an agreement"@en ;
    skos:inScheme p7012:process-classes ;
    skos:prefLabel "Agreement Negotiation"@en .

p7012:AgreementNegotiationClarificationRequired a rdfs:Class,
        skos:Concept,
        p7012:AgreementNegotiationStatus ;
    dct:created "2024-12-17"^^xsd:date ;
    rdfs:isDefinedBy p7012: ;
    sw:term_status "accepted"@en ;
    skos:broader p7012:AgreementNegotiationStatus ;
    skos:definition "Status indicating the Agreement Negotiation requires a clarification from the other party regarding the relevant context"@en ;
    skos:inScheme p7012:status-classes ;
    skos:prefLabel "Agreement Negotiation Clarification Required"@en .

p7012:AgreementNegotiationConfirmationRequired a rdfs:Class,
        skos:Concept,
        p7012:AgreementNegotiationStatus ;
    dct:created "2024-12-17"^^xsd:date ;
    rdfs:isDefinedBy p7012: ;
    sw:term_status "accepted"@en ;
    skos:broader p7012:AgreementNegotiationStatus ;
    skos:definition "Status indicating the Agreement Negotiation requires a confirmation by a human before it can proceed"@en ;
    skos:inScheme p7012:status-classes ;
    skos:prefLabel "Agreement Negotiation Confirmation Required"@en .

p7012:AgreementNegotiationCounterOfferMade a rdfs:Class,
        skos:Concept,
        p7012:AgreementNegotiationStatus ;
    dct:created "2024-12-17"^^xsd:date ;
    rdfs:isDefinedBy p7012: ;
    sw:term_status "accepted"@en ;
    skos:broader p7012:AgreementNegotiationStatus ;
    skos:definition "Status indicating the terms involved in Agreement Negotiation were not accepted and a counter-offer has been made with a different set of terms"@en ;
    skos:inScheme p7012:status-classes ;
    skos:prefLabel "Agreement Negotiation Counter Offer Made"@en .

p7012:AgreementNegotiationExpired a rdfs:Class,
        skos:Concept,
        p7012:AgreementNegotiationStatus ;
    dct:created "2024-12-17"^^xsd:date ;
    rdfs:isDefinedBy p7012: ;
    sw:term_status "accepted"@en ;
    skos:broader p7012:AgreementNegotiationStatus ;
    skos:definition "Status indicating the Agreement Negotiation has expired due to inactivity by a party or due to other reasons"@en ;
    skos:inScheme p7012:status-classes ;
    skos:prefLabel "Agreement Negotiation Expired"@en .

p7012:AgreementNegotiationInitiated a rdfs:Class,
        skos:Concept,
        p7012:AgreementNegotiationStatus ;
    dct:created "2024-12-17"^^xsd:date ;
    rdfs:isDefinedBy p7012: ;
    sw:term_status "accepted"@en ;
    skos:broader p7012:AgreementNegotiationStatus ;
    skos:definition "Status indicating the Agreement Negotiation process has been initiated"@en ;
    skos:inScheme p7012:status-classes ;
    skos:prefLabel "Agreement Negotiation Initiated"@en .

p7012:AgreementNegotiationInvalid a rdfs:Class,
        skos:Concept,
        p7012:AgreementNegotiationStatus ;
    dct:created "2024-12-17"^^xsd:date ;
    rdfs:isDefinedBy p7012: ;
    sw:term_status "accepted"@en ;
    skos:broader p7012:AgreementNegotiationStatus ;
    skos:definition "Status indicating the Agreement Negotiation is deemed to be invalid and therefore cannot continue"@en ;
    skos:inScheme p7012:status-classes ;
    skos:prefLabel "Agreement Negotiation Invalid"@en .

p7012:AgreementNegotiationPaused a rdfs:Class,
        skos:Concept,
        p7012:AgreementNegotiationStatus ;
    dct:created "2024-12-17"^^xsd:date ;
    rdfs:isDefinedBy p7012: ;
    sw:term_status "accepted"@en ;
    skos:broader p7012:AgreementNegotiationStatus ;
    skos:definition "Status indicating the Agreement Negotiation has been paused i.e. halted or put on hold without a specific decision"@en ;
    skos:inScheme p7012:status-classes ;
    skos:prefLabel "Agreement Negotiation Paused"@en .

p7012:AgreementNegotiationPendingResponse a rdfs:Class,
        skos:Concept,
        p7012:AgreementNegotiationStatus ;
    dct:created "2024-12-17"^^xsd:date ;
    rdfs:isDefinedBy p7012: ;
    sw:term_status "accepted"@en ;
    skos:broader p7012:AgreementNegotiationStatus ;
    skos:definition "Status indicating the Agreement Negotiation process is underway and is awaiting a response from the other party"@en ;
    skos:inScheme p7012:status-classes ;
    skos:prefLabel "Agreement Negotiation Pending Response"@en .

p7012:AgreementNegotiationRefused a rdfs:Class,
        skos:Concept,
        p7012:AgreementNegotiationStatus ;
    dct:created "2024-12-17"^^xsd:date ;
    rdfs:isDefinedBy p7012: ;
    sw:term_status "accepted"@en ;
    skos:broader p7012:AgreementNegotiationStatus ;
    skos:definition "Status indicating the Agreement Negotiation has been refused to be initiated or continued"@en ;
    skos:inScheme p7012:status-classes ;
    skos:prefLabel "Agreement Negotiation Refused"@en .

p7012:AgreementNegotiationRequest a rdfs:Class,
        skos:Concept ;
    dct:created "2024-12-17"^^xsd:date ;
    rdfs:isDefinedBy p7012: ;
    rdfs:subClassOf dpv:Process ;
    sw:term_status "accepted"@en ;
    skos:broader dpv:Process ;
    skos:definition "A request to initiate negotiation with the goal of finding an acceptable agreement"@en ;
    skos:inScheme p7012:process-classes ;
    skos:prefLabel "Agreement Negotiation Request"@en .

p7012:AgreementNegotiationRequested a rdfs:Class,
        skos:Concept,
        p7012:AgreementNegotiationStatus ;
    dct:created "2024-12-17"^^xsd:date ;
    rdfs:isDefinedBy p7012: ;
    sw:term_status "accepted"@en ;
    skos:broader p7012:AgreementNegotiationStatus ;
    skos:definition "Status indicating the Agreement Negotiation has been requested to be initiated"@en ;
    skos:inScheme p7012:status-classes ;
    skos:prefLabel "Agreement Negotiation Requested"@en .

p7012:AgreementNegotiationStatus a rdfs:Class,
        skos:Concept ;
    dct:created "2024-12-17"^^xsd:date ;
    rdfs:isDefinedBy p7012: ;
    rdfs:subClassOf dpv:Status ;
    sw:term_status "accepted"@en ;
    skos:broader dpv:Status ;
    skos:definition "Status associated with the Agreement Negotiation"@en ;
    skos:inScheme p7012:status-classes ;
    skos:prefLabel "Agreement Negotiation Status"@en .

p7012:AgreementNegotiationTerminated a rdfs:Class,
        skos:Concept,
        p7012:AgreementNegotiationStatus ;
    dct:created "2024-12-17"^^xsd:date ;
    rdfs:isDefinedBy p7012: ;
    sw:term_status "accepted"@en ;
    skos:broader p7012:AgreementNegotiationStatus ;
    skos:definition "Status indicating the Agreement Negotiation has been terminated by one or more parties"@en ;
    skos:inScheme p7012:status-classes ;
    skos:prefLabel "Agreement Negotiation Terminated"@en .

p7012:AgreementNegotiationUnknown a rdfs:Class,
        skos:Concept,
        p7012:AgreementNegotiationStatus ;
    dct:created "2024-12-17"^^xsd:date ;
    rdfs:isDefinedBy p7012: ;
    sw:term_status "accepted"@en ;
    skos:broader p7012:AgreementNegotiationStatus ;
    skos:definition "Status indicating the state of Agreement Negotiation is unknown"@en ;
    skos:inScheme p7012:status-classes ;
    skos:prefLabel "Agreement Negotiation Unknown"@en .

p7012:AgreementPreference a rdfs:Class,
        skos:Concept ;
    dct:created "2024-12-17"^^xsd:date ;
    rdfs:isDefinedBy p7012: ;
    rdfs:subClassOf dpv:Rule ;
    sw:term_status "accepted"@en ;
    skos:broader dpv:Rule ;
    skos:definition "A preference regarding agreements, such as to indicate which terms are acceptable or unacceptable"@en ;
    skos:inScheme p7012:process-classes ;
    skos:prefLabel "Agreement Preference"@en .

p7012:AgreementRefused a rdfs:Class,
        skos:Concept,
        p7012:AgreementNegotiationStatus ;
    dct:created "2024-12-17"^^xsd:date ;
    rdfs:isDefinedBy p7012: ;
    sw:term_status "accepted"@en ;
    skos:broader p7012:AgreementNegotiationStatus ;
    skos:definition "Status indicating the Agreement Negotiation is completed and the parties have refused the relevant terms"@en ;
    skos:inScheme p7012:status-classes ;
    skos:prefLabel "Agreement Refused"@en .

p7012:AgreementRegistry a rdfs:Class,
        skos:Concept ;
    dct:created "2024-12-17"^^xsd:date ;
    rdfs:isDefinedBy p7012: ;
    sw:term_status "accepted"@en ;
    skos:definition "A registry hosting agreements that acts as a common repository for parties to utilise as a reference within requests and for negotiating acceptable terms"@en ;
    skos:inScheme p7012:process-classes ;
    skos:prefLabel "Agreement Term Registry"@en .

p7012:ConflictResolutionTerm a rdfs:Class,
        skos:Concept ;
    dct:created "2024-12-17"^^xsd:date ;
    rdfs:isDefinedBy p7012: ;
    rdfs:subClassOf dpv:ContractualClause ;
    sw:term_status "accepted"@en ;
    skos:broader dpv:ContractualClause ;
    skos:definition "Term related to resolving conflicts in Term(s)"@en ;
    skos:inScheme p7012:privacy-term-classes ;
    skos:prefLabel "Conflict Resolution Term"@en .

p7012:DataSharingTerm a rdfs:Class,
        skos:Concept ;
    dct:created "2024-12-17"^^xsd:date ;
    rdfs:isDefinedBy p7012: ;
    rdfs:subClassOf dpv:ContractualClause ;
    sw:term_status "accepted"@en ;
    skos:broader dpv:ContractualClause ;
    skos:definition "Term related to Data Sharing"@en ;
    skos:inScheme p7012:privacy-term-classes ;
    skos:prefLabel "Data Sharing Term"@en .

p7012:DataTransparencyExAnte a rdfs:Class,
        skos:Concept,
        dpv:Obligation,
        p7012:DataTransparencyTerm ;
    dct:created "2024-12-17"^^xsd:date ;
    rdfs:isDefinedBy p7012: ;
    sw:term_status "accepted"@en ;
    skos:broader p7012:DataTransparencyRequired ;
    skos:definition "Term that indicates transparency regarding data involved and its source is obligated ahead of intended process i.e. ex-ante transparency regarding data involved and its source"@en ;
    skos:inScheme p7012:privacy-term-classes ;
    skos:prefLabel "Data Transparency Ex Ante"@en .

p7012:DataTransparencyExPost a rdfs:Class,
        skos:Concept,
        dpv:Obligation,
        p7012:DataTransparencyTerm ;
    dct:created "2024-12-17"^^xsd:date ;
    rdfs:isDefinedBy p7012: ;
    sw:term_status "accepted"@en ;
    skos:broader p7012:DataTransparencyRequired ;
    skos:definition "Term that indicates transparency regarding data involved and its source is obligated after intended process i.e. ex-post transparency regarding data involved and its source"@en ;
    skos:inScheme p7012:privacy-term-classes ;
    skos:prefLabel "Data Transparency Ex Post"@en .

p7012:DataTransparencyNotRequired a rdfs:Class,
        skos:Concept,
        p7012:DataTransparencyTerm ;
    dct:created "2024-12-17"^^xsd:date ;
    rdfs:isDefinedBy p7012: ;
    sw:term_status "accepted"@en ;
    skos:broader p7012:DataTransparencyTerm ;
    skos:definition "Term that indicates transparency regarding data involved and its source is not required to be provided"@en ;
    skos:inScheme p7012:privacy-term-classes ;
    skos:prefLabel "Data Transparency Not Required"@en .

p7012:DataTransparencyOnRequest a rdfs:Class,
        skos:Concept,
        dpv:Obligation,
        p7012:DataTransparencyTerm ;
    dct:created "2024-12-17"^^xsd:date ;
    rdfs:isDefinedBy p7012: ;
    sw:term_status "accepted"@en ;
    skos:broader p7012:DataTransparencyRequired ;
    skos:definition "Term that indicates transparency regarding data involved and its source is obligated upon request"@en ;
    skos:inScheme p7012:privacy-term-classes ;
    skos:prefLabel "Data Transparency On Request"@en .

p7012:DataTransparencyRequired a rdfs:Class,
        skos:Concept,
        dpv:Obligation,
        p7012:DataTransparencyTerm ;
    dct:created "2024-12-17"^^xsd:date ;
    rdfs:isDefinedBy p7012: ;
    sw:term_status "accepted"@en ;
    skos:broader dpv:Obligation,
        p7012:DataTransparencyTerm ;
    skos:definition "Term that indicates transparency regarding data involved and its source is obligated"@en ;
    skos:inScheme p7012:privacy-term-classes ;
    skos:prefLabel "Data Transparency Required"@en .

p7012:DataTransparencyTerm a rdfs:Class,
        skos:Concept ;
    dct:created "2024-12-17"^^xsd:date ;
    rdfs:isDefinedBy p7012: ;
    rdfs:subClassOf p7012:TransparencyTerm ;
    sw:term_status "accepted"@en ;
    skos:broader p7012:TransparencyTerm ;
    skos:definition "Term that indicates transparency regarding data involved and its source as an obligation"@en ;
    skos:inScheme p7012:privacy-term-classes ;
    skos:prefLabel "Data Transparency Term"@en .

p7012:DeonticInterpretationTerm a rdfs:Class,
        skos:Concept ;
    dct:created "2024-12-17"^^xsd:date ;
    rdfs:isDefinedBy p7012: ;
    rdfs:subClassOf dpv:ContractualClause ;
    sw:term_status "accepted"@en ;
    skos:broader dpv:ContractualClause ;
    skos:definition "Term related to interpretation of the Term(s) using deontic logic"@en ;
    skos:inScheme p7012:privacy-term-classes ;
    skos:prefLabel "Deontic Interpretation Term"@en .

p7012:Entity a rdfs:Class,
        skos:Concept ;
    dct:created "2024-12-17"^^xsd:date ;
    rdfs:isDefinedBy p7012: ;
    rdfs:subClassOf dpv:Organisation ;
    sw:term_status "accepted"@en ;
    skos:broader dpv:Organisation ;
    skos:definition "An entity is any organisation with which a person makes or intends to make a contractual agreement, and which is the second party in a contract"@en ;
    skos:inScheme p7012:entities-classes ;
    skos:prefLabel "Entityi"@en .

p7012:EntityAgent a rdfs:Class,
        skos:Concept ;
    dct:created "2024-12-17"^^xsd:date ;
    rdfs:isDefinedBy p7012: ;
    rdfs:subClassOf p7012:Agent ;
    sw:term_status "accepted"@en ;
    skos:broader p7012:Agent ;
    skos:definition "An Agent that repersents the Entity"@en ;
    skos:inScheme p7012:entities-classes ;
    skos:prefLabel "Entity Agent"@en .

p7012:NonServiceData a rdfs:Class,
        skos:Concept,
        dpv:PersonalData ;
    dct:created "2024-12-17"^^xsd:date ;
    rdfs:isDefinedBy p7012: ;
    sw:term_status "accepted"@en ;
    skos:broader dpv:PersonalData ;
    skos:definition "Data other than what is collected, produced, or otherwise generated in the context of a Service"@en ;
    skos:inScheme p7012:data-classes ;
    skos:prefLabel "Non-Service Data"@en .

p7012:P7012Endpoint a rdfs:Class,
        skos:Concept ;
    dct:created "2024-12-17"^^xsd:date ;
    rdfs:isDefinedBy p7012: ;
    rdfs:subClassOf dpv:Location ;
    sw:term_status "accepted"@en ;
    skos:broader dpv:Location ;
    skos:definition "A location that acts as an endpoint, such as a URL, for carrying out communications and interactions between parties as defined in P7012"@en ;
    skos:inScheme p7012:process-classes ;
    skos:prefLabel "P7012 Endpoint"@en .

p7012:PDC a rdfs:Class,
        skos:Concept ;
    dct:created "2024-12-17"^^xsd:date ;
    rdfs:isDefinedBy p7012: ;
    sw:term_status "accepted"@en ;
    skos:definition "Term that indicates access is proactively provided by the person"@en ;
    skos:inScheme p7012:agreement-classes ;
    skos:prefLabel "Personal Data Contribution"@en .

p7012:PDC-AI a rdfs:Class,
        skos:Concept,
        p7012:Agreement ;
    dct:created "2024-12-17"^^xsd:date ;
    rdfs:isDefinedBy p7012: ;
    sw:term_status "accepted"@en ;
    skos:broader p7012:PDC ;
    skos:definition "Term that indicates access to data is being provided for the purposes of Training and Operating AI technologies"@en ;
    skos:inScheme p7012:agreement-classes ;
    skos:prefLabel "Personal Data Contribution for AI Training and Development"@en .

p7012:PDC-GOOD a rdfs:Class,
        skos:Concept,
        p7012:Agreement ;
    dct:created "2024-12-17"^^xsd:date ;
    rdfs:isDefinedBy p7012: ;
    sw:term_status "accepted"@en ;
    skos:broader p7012:PDC ;
    skos:definition "Term that indicates access to data is being provided for the purposes of Public Good"@en ;
    skos:inScheme p7012:agreement-classes ;
    skos:prefLabel "Personal Data Contribution for Public Good"@en .

p7012:PDC-INTENT a rdfs:Class,
        skos:Concept,
        p7012:Agreement ;
    dct:created "2024-12-17"^^xsd:date ;
    rdfs:isDefinedBy p7012: ;
    sw:term_status "accepted"@en ;
    skos:broader p7012:PDC ;
    skos:definition "Term that indicates access to data is being provided for the purposes of Intent Casting"@en ;
    skos:inScheme p7012:agreement-classes ;
    skos:prefLabel "Personal Data Contribution for Intent Casting"@en .

p7012:PartyTransparencyExAnte a rdfs:Class,
        skos:Concept,
        dpv:Obligation,
        p7012:PartyTransparencyTerm ;
    dct:created "2024-12-17"^^xsd:date ;
    rdfs:isDefinedBy p7012: ;
    sw:term_status "accepted"@en ;
    skos:broader p7012:PartyTransparencyRequired ;
    skos:definition "Term that indicates transparency regarding identities and involvement of parties in specific roles is obligated ahead of intended process i.e. ex-ante transparency regarding identities and involvement of parties in specific roles"@en ;
    skos:inScheme p7012:privacy-term-classes ;
    skos:prefLabel "Party Transparency Ex Ante"@en .

p7012:PartyTransparencyExPost a rdfs:Class,
        skos:Concept,
        dpv:Obligation,
        p7012:PartyTransparencyTerm ;
    dct:created "2024-12-17"^^xsd:date ;
    rdfs:isDefinedBy p7012: ;
    sw:term_status "accepted"@en ;
    skos:broader p7012:PartyTransparencyRequired ;
    skos:definition "Term that indicates transparency regarding identities and involvement of parties in specific roles is obligated after intended process i.e. ex-post transparency regarding identities and involvement of parties in specific roles"@en ;
    skos:inScheme p7012:privacy-term-classes ;
    skos:prefLabel "Party Transparency Ex Post"@en .

p7012:PartyTransparencyNotRequired a rdfs:Class,
        skos:Concept,
        p7012:PartyTransparencyTerm ;
    dct:created "2024-12-17"^^xsd:date ;
    rdfs:isDefinedBy p7012: ;
    sw:term_status "accepted"@en ;
    skos:broader p7012:PartyTransparencyTerm ;
    skos:definition "Term that indicates transparency regarding identities and involvement of parties in specific roles is not required to be provided"@en ;
    skos:inScheme p7012:privacy-term-classes ;
    skos:prefLabel "Party Transparency Not Required"@en .

p7012:PartyTransparencyOnRequest a rdfs:Class,
        skos:Concept,
        dpv:Obligation,
        p7012:PartyTransparencyTerm ;
    dct:created "2024-12-17"^^xsd:date ;
    rdfs:isDefinedBy p7012: ;
    sw:term_status "accepted"@en ;
    skos:broader p7012:PartyTransparencyRequired ;
    skos:definition "Term that indicates transparency regarding identities and involvement of parties in specific roles is obligated upon request"@en ;
    skos:inScheme p7012:privacy-term-classes ;
    skos:prefLabel "Party Transparency On Request"@en .

p7012:PartyTransparencyRequired a rdfs:Class,
        skos:Concept,
        dpv:Obligation,
        p7012:PartyTransparencyTerm ;
    dct:created "2024-12-17"^^xsd:date ;
    rdfs:isDefinedBy p7012: ;
    sw:term_status "accepted"@en ;
    skos:broader dpv:Obligation,
        p7012:PartyTransparencyTerm ;
    skos:definition "Term that indicates transparency regarding identities and involvement of parties in specific roles is obligated"@en ;
    skos:inScheme p7012:privacy-term-classes ;
    skos:prefLabel "Party Transparency Required"@en .

p7012:PartyTransparencyTerm a rdfs:Class,
        skos:Concept ;
    dct:created "2024-12-17"^^xsd:date ;
    rdfs:isDefinedBy p7012: ;
    rdfs:subClassOf p7012:TransparencyTerm ;
    sw:term_status "accepted"@en ;
    skos:broader p7012:TransparencyTerm ;
    skos:definition "Term that indicates transparency regarding identities and involvement of parties in specific roles as an obligation"@en ;
    skos:inScheme p7012:privacy-term-classes ;
    skos:prefLabel "Party Transparency Term"@en .

p7012:PermissiveInterpretation a rdfs:Class,
        skos:Concept,
        p7012:DeonticInterpretationTerm ;
    dct:created "2024-12-17"^^xsd:date ;
    rdfs:isDefinedBy p7012: ;
    sw:term_status "accepted"@en ;
    skos:broader p7012:DeonticInterpretationTerm ;
    skos:definition "Term that indicates a permissive interpretation where if something is not prohibited or if there are no rules governing it, then it is assumed to be permitted"@en ;
    skos:inScheme p7012:privacy-term-classes ;
    skos:prefLabel "Permissive Interpretation"@en .

p7012:Person a rdfs:Class,
        skos:Concept ;
    dct:created "2024-12-17"^^xsd:date ;
    rdfs:isDefinedBy p7012: ;
    rdfs:subClassOf dpv:NaturalPerson ;
    sw:term_status "accepted"@en ;
    skos:broader dpv:NaturalPerson ;
    skos:definition "The human individual or person whose personal data or privacy is involved, and which is the first party in a contract"@en ;
    skos:inScheme p7012:entities-classes ;
    skos:prefLabel "Person"@en .

p7012:PersonAgent a rdfs:Class,
        skos:Concept ;
    dct:created "2024-12-17"^^xsd:date ;
    rdfs:isDefinedBy p7012: ;
    rdfs:subClassOf p7012:Agent ;
    sw:term_status "accepted"@en ;
    skos:broader p7012:Agent ;
    skos:definition "An Agent that represents the Person"@en ;
    skos:inScheme p7012:entities-classes ;
    skos:prefLabel "Person Agent"@en .

p7012:PortabilityNotRequired a rdfs:Class,
        skos:Concept,
        dpv:Obligation,
        p7012:PortabilityTerm ;
    dct:created "2024-12-17"^^xsd:date ;
    rdfs:isDefinedBy p7012: ;
    sw:term_status "accepted"@en ;
    skos:broader dpv:Obligation,
        p7012:PortabilityTerm ;
    skos:definition "Term that indicates data portability is not required to be provided"@en ;
    skos:inScheme p7012:privacy-term-classes ;
    skos:prefLabel "Portability Not Required"@en .

p7012:PortabilityRequired a rdfs:Class,
        skos:Concept,
        dpv:Obligation,
        p7012:PortabilityTerm ;
    dct:created "2024-12-17"^^xsd:date ;
    rdfs:isDefinedBy p7012: ;
    sw:term_status "accepted"@en ;
    skos:broader dpv:Obligation,
        p7012:PortabilityTerm ;
    skos:definition "Term that indicates data portability is required to be provided"@en ;
    skos:inScheme p7012:privacy-term-classes ;
    skos:prefLabel "Portability Required"@en .

p7012:PortabilityRequiredImmediately a rdfs:Class,
        skos:Concept,
        dpv:Obligation,
        p7012:PortabilityTerm ;
    dct:created "2024-12-17"^^xsd:date ;
    rdfs:isDefinedBy p7012: ;
    sw:term_status "accepted"@en ;
    skos:broader p7012:PortabilityRequired ;
    skos:definition "Term that indicates data should be ported or made available immediately without delay"@en ;
    skos:inScheme p7012:privacy-term-classes ;
    skos:prefLabel "Portability Required Immediately"@en .

p7012:PortabilityRequiredOnRequest a rdfs:Class,
        skos:Concept,
        dpv:Obligation,
        p7012:PortabilityTerm ;
    dct:created "2024-12-17"^^xsd:date ;
    rdfs:isDefinedBy p7012: ;
    sw:term_status "accepted"@en ;
    skos:broader p7012:PortabilityRequired ;
    skos:definition "Term that indicates data should be ported or made available on request"@en ;
    skos:inScheme p7012:privacy-term-classes ;
    skos:prefLabel "Portability Required On Request"@en .

p7012:PortabilityTerm a rdfs:Class,
        skos:Concept ;
    dct:created "2024-12-17"^^xsd:date ;
    rdfs:isDefinedBy p7012: ;
    rdfs:subClassOf dpv:ContractualClause ;
    sw:term_status "accepted"@en ;
    skos:broader dpv:ContractualClause ;
    skos:definition "Term that indicates portability of data from service provider to individual"@en ;
    skos:inScheme p7012:privacy-term-classes ;
    skos:prefLabel "Portability Term"@en .

p7012:PortabilityToThirdParty a rdfs:Class,
        skos:Concept,
        dpv:Obligation,
        p7012:PortabilityTerm ;
    dct:created "2024-12-17"^^xsd:date ;
    rdfs:isDefinedBy p7012: ;
    sw:term_status "accepted"@en ;
    skos:broader p7012:PortabilityRequired ;
    skos:definition "Term that indicates data should be ported or made available to third party"@en ;
    skos:inScheme p7012:privacy-term-classes ;
    skos:prefLabel "Portability To Third Party"@en .

p7012:PreferenceAlwaysApplies a rdfs:Class,
        skos:Concept,
        p7012:PreferenceApplicability ;
    dct:created "2024-12-17"^^xsd:date ;
    rdfs:isDefinedBy p7012: ;
    sw:term_status "accepted"@en ;
    skos:broader p7012:PreferenceApplicability ;
    skos:definition "Term that indicates the privacy preference always applies in all contexts and should always be used in agreements and negotiations"@en ;
    skos:inScheme p7012:privacy-term-classes ;
    skos:prefLabel "Preference Always Applies"@en .

p7012:PreferenceApplicability a rdfs:Class,
        skos:Concept ;
    dct:created "2024-12-17"^^xsd:date ;
    rdfs:isDefinedBy p7012: ;
    rdfs:subClassOf dpv:ContractualClause ;
    sw:term_status "accepted"@en ;
    skos:broader dpv:ContractualClause ;
    skos:definition "Term that indicates the applicability of Privacy Preference(s)"@en ;
    skos:inScheme p7012:privacy-term-classes ;
    skos:prefLabel "Privacy Preference Applicability"@en .

p7012:PreferenceConditionallyApplies a rdfs:Class,
        skos:Concept,
        p7012:PreferenceApplicability ;
    dct:created "2024-12-17"^^xsd:date ;
    rdfs:isDefinedBy p7012: ;
    sw:term_status "accepted"@en ;
    skos:broader p7012:PreferenceApplicability ;
    skos:definition "Term that indicates the privacy preference conditionally applies i.e. it should only be used in agreements and negotiations if the associated condition is satisfied within the context"@en ;
    skos:inScheme p7012:privacy-term-classes ;
    skos:prefLabel "Preference Conditionally Applies"@en .

p7012:PreferenceNeverApplies a rdfs:Class,
        skos:Concept,
        p7012:PreferenceApplicability ;
    dct:created "2024-12-17"^^xsd:date ;
    rdfs:isDefinedBy p7012: ;
    sw:term_status "accepted"@en ;
    skos:broader p7012:PreferenceApplicability ;
    skos:definition "Term that indicates the privacy preference never applies in any context and should never be used in agreements or negotiations"@en ;
    skos:inScheme p7012:privacy-term-classes ;
    skos:prefLabel "Preference Never Applies"@en .

p7012:Profiling2PAllowed a rdfs:Class,
        skos:Concept,
        dpv:Permission,
        p7012:ProfilingTerm ;
    dct:created "2024-12-17"^^xsd:date ;
    rdfs:isDefinedBy p7012: ;
    sw:term_status "accepted"@en ;
    skos:broader p7012:ProfilingAllowed ;
    skos:definition "Term that indicates Profiling is allowed but only by the 1st Party"@en ;
    skos:inScheme p7012:privacy-term-classes ;
    skos:prefLabel "Profiling Allowed Only First Party"@en .

p7012:Profiling3PDisallowed a rdfs:Class,
        skos:Concept,
        dpv:Prohibition,
        p7012:ProfilingTerm ;
    dct:created "2024-12-17"^^xsd:date ;
    rdfs:isDefinedBy p7012: ;
    sw:term_status "accepted"@en ;
    skos:broader p7012:ProfilingDisallowed ;
    skos:definition "Term that indicates Profiling is not allowed by 3rd Parties"@en ;
    skos:inScheme p7012:privacy-term-classes ;
    skos:prefLabel "Profiling Disallowed For Third Party"@en .

p7012:ProfilingAllowed a rdfs:Class,
        skos:Concept,
        dpv:Permission,
        p7012:ProfilingTerm ;
    dct:created "2024-12-17"^^xsd:date ;
    rdfs:isDefinedBy p7012: ;
    sw:term_status "accepted"@en ;
    skos:broader dpv:Permission,
        p7012:ProfilingTerm ;
    skos:definition "Term that indicates Profiling is allowed"@en ;
    skos:inScheme p7012:privacy-term-classes ;
    skos:prefLabel "Profiling Allowed"@en .

p7012:ProfilingDisallowed a rdfs:Class,
        skos:Concept,
        dpv:Prohibition,
        p7012:ProfilingTerm ;
    dct:created "2024-12-17"^^xsd:date ;
    rdfs:isDefinedBy p7012: ;
    sw:term_status "accepted"@en ;
    skos:broader dpv:Prohibition,
        p7012:ProfilingTerm ;
    skos:definition "Term that indicates Profiling is not allowed"@en ;
    skos:inScheme p7012:privacy-term-classes ;
    skos:prefLabel "Profiling Disallowed"@en .

p7012:ProfilingTerm a rdfs:Class,
        skos:Concept ;
    dct:created "2024-12-17"^^xsd:date ;
    rdfs:isDefinedBy p7012: ;
    rdfs:subClassOf dpv:ContractualClause ;
    sw:term_status "accepted"@en ;
    skos:broader dpv:ContractualClause ;
    skos:definition "Term related to Profiling"@en ;
    skos:inScheme p7012:privacy-term-classes ;
    skos:prefLabel "Profiling Term"@en .

p7012:ProfilingWithFPDisallowed a rdfs:Class,
        skos:Concept,
        dpv:Prohibition,
        p7012:ProfilingTerm ;
    dct:created "2024-12-17"^^xsd:date ;
    rdfs:isDefinedBy p7012: ;
    sw:term_status "accepted"@en ;
    skos:broader p7012:ProfilingDisallowed ;
    skos:definition "Term that indicates Profiling involving use of Fingerprinting is not allowed"@en ;
    skos:inScheme p7012:privacy-term-classes ;
    skos:prefLabel "Profiling Disallowed FP"@en .

p7012:ProfilingWithPIIDisallowed a rdfs:Class,
        skos:Concept,
        dpv:Prohibition,
        p7012:ProfilingTerm ;
    dct:created "2024-12-17"^^xsd:date ;
    rdfs:isDefinedBy p7012: ;
    sw:term_status "accepted"@en ;
    skos:broader p7012:ProfilingDisallowed ;
    skos:definition "Term that indicates Profiling involving use of PII is not allowed"@en ;
    skos:inScheme p7012:privacy-term-classes ;
    skos:prefLabel "Profiling Disallowed PII"@en .

p7012:ProfilingWithoutFPAllowed a rdfs:Class,
        skos:Concept,
        dpv:Permission,
        p7012:ProfilingTerm ;
    dct:created "2024-12-17"^^xsd:date ;
    rdfs:isDefinedBy p7012: ;
    sw:term_status "accepted"@en ;
    skos:broader p7012:ProfilingAllowed ;
    skos:definition "Term that indicates Profiling is allowed but only if it does not involve Fingerprinting"@en ;
    skos:inScheme p7012:privacy-term-classes ;
    skos:prefLabel "Profiling Allowed No FP"@en .

p7012:ProfilingWithoutPIIAllowed a rdfs:Class,
        skos:Concept,
        dpv:Permission,
        p7012:ProfilingTerm ;
    dct:created "2024-12-17"^^xsd:date ;
    rdfs:isDefinedBy p7012: ;
    sw:term_status "accepted"@en ;
    skos:broader p7012:ProfilingAllowed ;
    skos:definition "Term that indicates Profiling is allowed but only if it uses non-PII"@en ;
    skos:inScheme p7012:privacy-term-classes ;
    skos:prefLabel "Profiling Allowed Only Non PII"@en .

p7012:ProhibitiveInterpretation a rdfs:Class,
        skos:Concept,
        p7012:DeonticInterpretationTerm ;
    dct:created "2024-12-17"^^xsd:date ;
    rdfs:isDefinedBy p7012: ;
    sw:term_status "accepted"@en ;
    skos:broader p7012:DeonticInterpretationTerm ;
    skos:definition "Term that indicates a prohibitive interpretation where if something is not permitted or if there are no rules governing it, then it is assumed to be prohibited"@en ;
    skos:inScheme p7012:privacy-term-classes ;
    skos:prefLabel "Prohibitive Interpretation"@en .

p7012:PurposeTransparencyExAnte a rdfs:Class,
        skos:Concept,
        dpv:Obligation,
        p7012:PurposeTransparencyTerm ;
    dct:created "2024-12-17"^^xsd:date ;
    rdfs:isDefinedBy p7012: ;
    sw:term_status "accepted"@en ;
    skos:broader p7012:PurposeTransparencyRequired ;
    skos:definition "Term that indicates transparency regarding purposes involved for processing of data and technologies is obligated ahead of intended process i.e. ex-ante transparency regarding purposes involved for processing of data and technologies"@en ;
    skos:inScheme p7012:privacy-term-classes ;
    skos:prefLabel "Purpose Transparency Ex Ante"@en .

p7012:PurposeTransparencyExPost a rdfs:Class,
        skos:Concept,
        dpv:Obligation,
        p7012:PurposeTransparencyTerm ;
    dct:created "2024-12-17"^^xsd:date ;
    rdfs:isDefinedBy p7012: ;
    sw:term_status "accepted"@en ;
    skos:broader p7012:PurposeTransparencyRequired ;
    skos:definition "Term that indicates transparency regarding purposes involved for processing of data and technologies is obligated after intended process i.e. ex-post transparency regarding purposes involved for processing of data and technologies"@en ;
    skos:inScheme p7012:privacy-term-classes ;
    skos:prefLabel "Purpose Transparency Ex Post"@en .

p7012:PurposeTransparencyNotRequired a rdfs:Class,
        skos:Concept,
        p7012:PurposeTransparencyTerm ;
    dct:created "2024-12-17"^^xsd:date ;
    rdfs:isDefinedBy p7012: ;
    sw:term_status "accepted"@en ;
    skos:broader p7012:PurposeTransparencyTerm ;
    skos:definition "Term that indicates transparency regarding purposes involved for processing of data and technologies is not required to be provided"@en ;
    skos:inScheme p7012:privacy-term-classes ;
    skos:prefLabel "Purpose Transparency Not Required"@en .

p7012:PurposeTransparencyOnRequest a rdfs:Class,
        skos:Concept,
        dpv:Obligation,
        p7012:PurposeTransparencyTerm ;
    dct:created "2024-12-17"^^xsd:date ;
    rdfs:isDefinedBy p7012: ;
    sw:term_status "accepted"@en ;
    skos:broader p7012:PurposeTransparencyRequired ;
    skos:definition "Term that indicates transparency regarding purposes involved for processing of data and technologies is obligated upon request"@en ;
    skos:inScheme p7012:privacy-term-classes ;
    skos:prefLabel "Purpose Transparency On Request"@en .

p7012:PurposeTransparencyRequired a rdfs:Class,
        skos:Concept,
        dpv:Obligation,
        p7012:PurposeTransparencyTerm ;
    dct:created "2024-12-17"^^xsd:date ;
    rdfs:isDefinedBy p7012: ;
    sw:term_status "accepted"@en ;
    skos:broader dpv:Obligation,
        p7012:PurposeTransparencyTerm ;
    skos:definition "Term that indicates transparency regarding purposes is obligated"@en ;
    skos:inScheme p7012:privacy-term-classes ;
    skos:prefLabel "Purpose Transparency Required"@en .

p7012:PurposeTransparencyTerm a rdfs:Class,
        skos:Concept ;
    dct:created "2024-12-17"^^xsd:date ;
    rdfs:isDefinedBy p7012: ;
    rdfs:subClassOf p7012:TransparencyTerm ;
    sw:term_status "accepted"@en ;
    skos:broader p7012:TransparencyTerm ;
    skos:definition "Term that indicates transparency regarding purposes involved for processing of data and technologies as an obligation"@en ;
    skos:inScheme p7012:privacy-term-classes ;
    skos:prefLabel "Purpose Transparency Term"@en .

p7012:ResolveAcrossContexts a rdfs:Class,
        skos:Concept,
        p7012:ConflictResolutionTerm ;
    dct:created "2024-12-17"^^xsd:date ;
    rdfs:isDefinedBy p7012: ;
    sw:term_status "accepted"@en ;
    skos:broader p7012:ConflictResolutionTerm ;
    skos:definition "Term that indicates this conflict method should be used to resolve all conflicts across contexts i.e. other contexts that have their own conflict resolution method should be overridden"@en ;
    skos:inScheme p7012:privacy-term-classes ;
    skos:prefLabel "Resolve Across Contexts"@en .

p7012:ResolveByDiscarding a rdfs:Class,
        skos:Concept,
        p7012:ConflictResolutionTerm ;
    dct:created "2024-12-17"^^xsd:date ;
    rdfs:isDefinedBy p7012: ;
    sw:term_status "accepted"@en ;
    skos:broader p7012:ConflictResolutionTerm ;
    skos:definition "Term that indicates a conflict should be resolved by discarding the conflicting terms i.e. removing all terms that are in conflict"@en ;
    skos:inScheme p7012:privacy-term-classes ;
    skos:prefLabel "Resolve By Discarding"@en .

p7012:ResolveOnlyWithinContext a rdfs:Class,
        skos:Concept,
        p7012:ConflictResolutionTerm ;
    dct:created "2024-12-17"^^xsd:date ;
    rdfs:isDefinedBy p7012: ;
    sw:term_status "accepted"@en ;
    skos:broader p7012:ConflictResolutionTerm ;
    skos:definition "Term that indicates a conflict should be resolved using the specified method but only for this context i.e. other contexts that have their own conflict resolution method should not be overridden"@en ;
    skos:inScheme p7012:privacy-term-classes ;
    skos:prefLabel "Resolve Only Within Context"@en .

p7012:ResolvePreferringPermission a rdfs:Class,
        skos:Concept,
        p7012:ConflictResolutionTerm ;
    dct:created "2024-12-17"^^xsd:date ;
    rdfs:isDefinedBy p7012: ;
    sw:term_status "accepted"@en ;
    skos:broader p7012:ConflictResolutionTerm ;
    skos:definition "Term that indicates a conflict should be resolved by preferring the permission over the prohibition i.e. if something is both prohibited and permitted, it is assumed to be permitted"@en ;
    skos:inScheme p7012:privacy-term-classes ;
    skos:prefLabel "Resolve Preferring Permission"@en .

p7012:ResolvePreferringProhibition a rdfs:Class,
        skos:Concept,
        p7012:ConflictResolutionTerm ;
    dct:created "2024-12-17"^^xsd:date ;
    rdfs:isDefinedBy p7012: ;
    sw:term_status "accepted"@en ;
    skos:broader p7012:ConflictResolutionTerm ;
    skos:definition "Term that indicates a conflict should be resolved by preferring the prohibition over the permission i.e. if something is both prohibited and permitted, it is assumed to be prohibited"@en ;
    skos:inScheme p7012:privacy-term-classes ;
    skos:prefLabel "Resolve Preferring Prohibition"@en .

p7012:SD-BY a rdfs:Class,
        skos:Concept,
        p7012:Agreement ;
    dct:created "2024-12-17"^^xsd:date ;
    rdfs:isDefinedBy p7012: ;
    sw:term_status "accepted"@en ;
    skos:broader p7012:Agreement ;
    skos:definition "Term that requires Service Delivery, and prohibits Analytics, Tracking, or Profiling by 2nd and 3rd Party, and prohibits sharing any data with 3rd Party"@en ;
    skos:inScheme p7012:agreement-classes ;
    skos:prefLabel "SD-BY"@en ;
    dpv:hasObligation p7012:ServiceDeliveryRequired ;
    dpv:hasProhibition p7012:AnalyticsDisallowed,
        p7012:DataSharingDisallowed,
        p7012:ProfilingDisallowed,
        p7012:TrackingDisallowed .

p7012:SD-BY-A a rdfs:Class,
        skos:Concept,
        p7012:Agreement ;
    dct:created "2024-12-17"^^xsd:date ;
    rdfs:isDefinedBy p7012: ;
    sw:term_status "accepted"@en ;
    skos:broader p7012:SD-BY ;
    skos:definition "Term that requires Service Delivery and permits Analytics, and prohibits Analytics by 3rd Party, prohibits Tracking, or Profiling by 2nd and 3rd Party, and prohibits sharing any data with 3rd Party"@en ;
    skos:inScheme p7012:agreement-classes ;
    skos:prefLabel "SD BY-A"@en ;
    dpv:hasObligation p7012:ServiceDeliveryRequired ;
    dpv:hasPermission p7012:Analytics2PAllowed ;
    dpv:hasProhibition p7012:Analytics3PDisallowed,
        p7012:DataSharingDisallowed,
        p7012:ProfilingDisallowed,
        p7012:TrackingDisallowed .

p7012:SD-BY-A-DP a rdfs:Class,
        skos:Concept,
        p7012:Agreement ;
    dct:created "2024-12-17"^^xsd:date ;
    rdfs:isDefinedBy p7012: ;
    sw:term_status "accepted"@en ;
    skos:broader p7012:SD-BY-A,
        p7012:SD-BY-DP ;
    skos:definition "Term that requires Service Delivery and permits Analytics, with an obligation for Data Portability, and prohibits Analytics by 3rd Party, prohibits Tracking or Profiling by 2nd and 3rd Party, and prohibits sharing any data with 3rd Party"@en ;
    skos:inScheme p7012:agreement-classes ;
    skos:prefLabel "SD BY-A-DP"@en ;
    dpv:hasObligation p7012:PortabilityRequired,
        p7012:ServiceDeliveryRequired ;
    dpv:hasPermission p7012:Analytics2PAllowed ;
    dpv:hasProhibition p7012:Analytics3PDisallowed,
        p7012:DataSharingDisallowed,
        p7012:ProfilingDisallowed,
        p7012:TrackingDisallowed .

p7012:SD-BY-AT a rdfs:Class,
        skos:Concept,
        p7012:Agreement ;
    dct:created "2024-12-17"^^xsd:date ;
    rdfs:isDefinedBy p7012: ;
    sw:term_status "accepted"@en ;
    skos:broader p7012:SD-BY-A ;
    skos:definition "Term that requires Service Delivery, and permits Analytics and Tracking by the 2nd Party, and prohibits Analytics, or Tracking by 3rd Party, prohibits Profiling by 2nd and 3rd Party, and prohibits sharing any data with 3rd Party"@en ;
    skos:inScheme p7012:agreement-classes ;
    skos:prefLabel "SD BY-AT"@en ;
    dpv:hasObligation p7012:ServiceDeliveryRequired ;
    dpv:hasPermission p7012:Analytics2PAllowed,
        p7012:Tracking2PAllowed ;
    dpv:hasProhibition p7012:Analytics3PDisallowed,
        p7012:DataSharingDisallowed,
        p7012:ProfilingDisallowed,
        p7012:Tracking3PDisallowed .

p7012:SD-BY-AT-DP a rdfs:Class,
        skos:Concept,
        p7012:Agreement ;
    dct:created "2024-12-17"^^xsd:date ;
    rdfs:isDefinedBy p7012: ;
    sw:term_status "accepted"@en ;
    skos:broader p7012:SD-BY-AT,
        p7012:SD-BY-DP ;
    skos:definition "Term that requires Service Delivery, and permits Analytics and Tracking by the 2nd Party, with an obligation for Data Portability, and prohibits Analytics or Tracking by 3rd Party, prohibits Profiling by 2nd and 3rd Party, and prohibits sharing any data with 3rd Party"@en ;
    skos:inScheme p7012:agreement-classes ;
    skos:prefLabel "SD BY-AT-DP"@en ;
    dpv:hasObligation p7012:PortabilityRequired,
        p7012:ServiceDeliveryRequired ;
    dpv:hasPermission p7012:Analytics2PAllowed,
        p7012:Tracking2PAllowed ;
    dpv:hasProhibition p7012:Analytics3PDisallowed,
        p7012:DataSharingDisallowed,
        p7012:ProfilingDisallowed,
        p7012:Tracking3PDisallowed .

p7012:SD-BY-ATP a rdfs:Class,
        skos:Concept,
        p7012:Agreement ;
    dct:created "2024-12-17"^^xsd:date ;
    rdfs:isDefinedBy p7012: ;
    sw:term_status "accepted"@en ;
    skos:broader p7012:SD-BY-AT ;
    skos:definition "Term that requires Service Delivery, and permits Analytics, Tracking, or Profiling by the 2nd party, and prohibits Analytics, Tracking, or Profiling by 3rd Party, and prohibits sharing any data with 3rd Party"@en ;
    skos:inScheme p7012:agreement-classes ;
    skos:prefLabel "SD BY-ATP"@en ;
    dpv:hasObligation p7012:ServiceDeliveryRequired ;
    dpv:hasPermission p7012:Analytics2PAllowed,
        p7012:Profiling2PAllowed,
        <https://w3id.org/dpv/standards/p7012#Tracking2PAllowed
> ;
    dpv:hasProhibition p7012:Analytics3PDisallowed,
        p7012:DataSharingDisallowed,
        p7012:Profiling3PDisallowed,
        p7012:Tracking3PDisallowed .

p7012:SD-BY-ATP-DP a rdfs:Class,
        skos:Concept,
        p7012:Agreement ;
    dct:created "2024-12-17"^^xsd:date ;
    rdfs:isDefinedBy p7012: ;
    sw:term_status "accepted"@en ;
    skos:broader p7012:SD-BY-ATP,
        p7012:SD-BY-DP ;
    skos:definition "Term that requires Service Delivery, and permits Analytics, Tracking, or Profiling by the 2nd Party, with an obligation for Data Portability, and prohibits Analytics, Tracking, or Profiling by 3rd Party, and prohibits sharing any data with 3rd Party"@en ;
    skos:inScheme p7012:agreement-classes ;
    skos:prefLabel "SD BY-ATP-DP"@en ;
    dpv:hasObligation p7012:PortabilityRequired,
        p7012:ServiceDeliveryRequired ;
    dpv:hasPermission p7012:Analytics2PAllowed,
        p7012:Profiling2PAllowed,
        <https://w3id.org/dpv/standards/p7012#Tracking2PAllowed
> ;
    dpv:hasProhibition p7012:Analytics3PDisallowed,
        p7012:DataSharingDisallowed,
        p7012:Profiling3PDisallowed,
        p7012:Tracking3PDisallowed .

p7012:SD-BY-ATP-S3P a rdfs:Class,
        skos:Concept,
        p7012:Agreement ;
    dct:created "2024-12-17"^^xsd:date ;
    rdfs:isDefinedBy p7012: ;
    sw:term_status "accepted"@en ;
    skos:broader p7012:SD-BY-ATP ;
    skos:definition "Term that requires Service Delivery, and permits Analytics, Tracking, or Profiling by the 2nd Party, and permits sharing data that has been fully anonymised with 3rd Party, and prohibits Analytics, Tracking, or Profiling by 3rd Party, and prohibits sharing on non-anonymised data with 3rd Party"@en ;
    skos:inScheme p7012:agreement-classes ;
    skos:prefLabel "SD BY-ATP-S3P"@en ;
    dpv:hasObligation p7012:ServiceDeliveryRequired ;
    dpv:hasPermission p7012:Analytics2PAllowed,
        p7012:DataSharingAnonymised3PAllowed,
        p7012:Profiling2PAllowed,
        <https://w3id.org/dpv/standards/p7012#Tracking2PAllowed
> ;
    dpv:hasProhibition p7012:Analytics3PDisallowed,
        p7012:Profiling3PDisallowed,
        p7012:SharingDataNonAnonymised3PDisallowed,
        p7012:Tracking3PDisallowed .

p7012:SD-BY-ATP-S3P-DP a rdfs:Class,
        skos:Concept,
        p7012:Agreement ;
    dct:created "2024-12-17"^^xsd:date ;
    rdfs:isDefinedBy p7012: ;
    sw:term_status "accepted"@en ;
    skos:broader p7012:SD-BY-ATP-S3P,
        p7012:SD-BY-DP ;
    skos:definition "Term that requires Service Delivery, and permits Analytics, Tracking, or Profiling by the 2nd Party, and permits sharing data that has been fully anonymised with 3rd Party, with an obligation for Data Portability, and prohibits Analytics, Tracking, Profiling by 3rd Party, and prohibits sharing on non-anonymised data with 3rd Party"@en ;
    skos:inScheme p7012:agreement-classes ;
    skos:prefLabel "SD BY-ATP-S3P-DP"@en ;
    dpv:hasObligation p7012:PortabilityRequired,
        p7012:ServiceDeliveryRequired ;
    dpv:hasPermission p7012:Analytics2PAllowed,
        p7012:DataSharingAnonymised3PAllowed,
        p7012:Profiling2PAllowed,
        <https://w3id.org/dpv/standards/p7012#Tracking2PAllowed
> ;
    dpv:hasProhibition p7012:Analytics3PDisallowed,
        p7012:Profiling3PDisallowed,
        p7012:SharingDataNonAnonymised3PDisallowed,
        p7012:Tracking3PDisallowed .

p7012:SD-BY-DP a rdfs:Class,
        skos:Concept,
        p7012:Agreement ;
    dct:created "2024-12-17"^^xsd:date ;
    rdfs:isDefinedBy p7012: ;
    sw:term_status "accepted"@en ;
    skos:broader p7012:SD-BY ;
    skos:definition "Term that requires Service Delivery, with an obligation for Data Portability, and prohibits Analytics, Tracking, or Profiling by 2nd and 3rd Party, and prohibits sharing any data with 3rd Party"@en ;
    skos:inScheme p7012:agreement-classes ;
    skos:prefLabel "SD BY-DP"@en ;
    dpv:hasObligation p7012:PortabilityRequired,
        p7012:ServiceDeliveryRequired ;
    dpv:hasProhibition p7012:AnalyticsDisallowed,
        p7012:DataSharingDisallowed,
        p7012:ProfilingDisallowed,
        p7012:TrackingDisallowed .

p7012:ServiceAnalytics a rdfs:Class,
        skos:Concept,
        dpv:Purpose ;
    dct:created "2024-12-17"^^xsd:date ;
    rdfs:isDefinedBy p7012: ;
    sw:term_status "accepted"@en ;
    skos:broader dpv:Purpose ;
    skos:definition "Purposes associated with analysing the usage, delivery, and provisioning metrics of a service"@en ;
    skos:inScheme p7012:purpose-classes ;
    skos:prefLabel "Service Analytics"@en .

p7012:ServiceAnalyticsData a rdfs:Class,
        skos:Concept,
        dpv:PersonalData ;
    dct:created "2024-12-17"^^xsd:date ;
    rdfs:isDefinedBy p7012: ;
    sw:term_status "accepted"@en ;
    skos:broader dpv:PersonalData ;
    skos:definition "Data collected, produced, or otherwise generated in the context of analysing the usage and provision of a Service"@en ;
    skos:inScheme p7012:data-classes ;
    skos:prefLabel "Service Analytics Data"@en .

p7012:ServiceData a rdfs:Class,
        skos:Concept,
        dpv:PersonalData ;
    dct:created "2024-12-17"^^xsd:date ;
    rdfs:isDefinedBy p7012: ;
    sw:term_status "accepted"@en ;
    skos:broader dpv:PersonalData ;
    skos:definition "Data collected, produced, or otherwise generated in the context of a Service"@en ;
    skos:inScheme p7012:data-classes ;
    skos:prefLabel "Service Data"@en .

p7012:ServiceDelivery a rdfs:Class,
        skos:Concept,
        dpv:Purpose ;
    dct:created "2024-12-17"^^xsd:date ;
    rdfs:isDefinedBy p7012: ;
    sw:term_status "accepted"@en ;
    skos:broader dpv:Purpose ;
    skos:definition "Purposes associated with delivery of a service"@en ;
    skos:inScheme p7012:purpose-classes ;
    skos:prefLabel "Service Delivery"@en .

p7012:ServiceImprovement a rdfs:Class,
        skos:Concept,
        dpv:Purpose ;
    dct:created "2024-12-17"^^xsd:date ;
    rdfs:isDefinedBy p7012: ;
    sw:term_status "accepted"@en ;
    skos:broader dpv:Purpose ;
    skos:definition "Purposes associated with identifying and implementing improvements to a service"@en ;
    skos:inScheme p7012:purpose-classes ;
    skos:prefLabel "Service Improvement"@en .

p7012:ServiceUsageData a rdfs:Class,
        skos:Concept,
        dpv:PersonalData ;
    dct:created "2024-12-17"^^xsd:date ;
    rdfs:isDefinedBy p7012: ;
    sw:term_status "accepted"@en ;
    skos:broader dpv:PersonalData ;
    skos:definition "Data collected, produced, or otherwise generated in the context of using a Service"@en ;
    skos:inScheme p7012:data-classes ;
    skos:prefLabel "Service Usage Data"@en .

p7012:SharingData3PAllowed a rdfs:Class,
        skos:Concept,
        dpv:Permission,
        p7012:DataSharingTerm ;
    dct:created "2024-12-17"^^xsd:date ;
    rdfs:isDefinedBy p7012: ;
    sw:term_status "accepted"@en ;
    skos:broader p7012:SharingDataAllowed ;
    skos:definition "Term that indicates data sharing with third party is allowed"@en ;
    skos:inScheme p7012:privacy-term-classes ;
    skos:prefLabel "Sharing Data with 3rd Party Allowed"@en .

p7012:SharingData3PDisallowed a rdfs:Class,
        skos:Concept,
        dpv:Prohibition,
        p7012:DataSharingTerm ;
    dct:created "2024-12-17"^^xsd:date ;
    rdfs:isDefinedBy p7012: ;
    sw:term_status "accepted"@en ;
    skos:broader p7012:SharingDataDisallowed ;
    skos:definition "Term that indicates data sharing with third party is disallowed"@en ;
    skos:inScheme p7012:privacy-term-classes ;
    skos:prefLabel "Sharing Data with 3rd Party Disallowed"@en .

p7012:SharingDataAllowed a rdfs:Class,
        skos:Concept,
        dpv:Permission,
        p7012:DataSharingTerm ;
    dct:created "2024-12-17"^^xsd:date ;
    rdfs:isDefinedBy p7012: ;
    sw:term_status "accepted"@en ;
    skos:broader dpv:Permission,
        p7012:DataSharingTerm ;
    skos:definition "Term that indicates Data Sharing is allowed"@en ;
    skos:inScheme p7012:privacy-term-classes ;
    skos:prefLabel "Sharing Data Allowed"@en .

p7012:SharingDataAnonymised3PAllowed a rdfs:Class,
        skos:Concept,
        dpv:Permission,
        p7012:DataSharingTerm ;
    dct:created "2024-12-17"^^xsd:date ;
    rdfs:isDefinedBy p7012: ;
    sw:term_status "accepted"@en ;
    skos:broader p7012:SharingDataAllowed ;
    skos:definition "Term that indicates data sharing only of anonymised data with third party is allowed"@en ;
    skos:inScheme p7012:privacy-term-classes ;
    skos:prefLabel "Sharing Anonymised Data with 3rd Party Allowed"@en .

p7012:SharingDataAnonymised3PDisallowed a rdfs:Class,
        skos:Concept,
        dpv:Prohibition,
        p7012:DataSharingTerm ;
    dct:created "2024-12-17"^^xsd:date ;
    rdfs:isDefinedBy p7012: ;
    sw:term_status "accepted"@en ;
    skos:broader p7012:SharingDataDisallowed ;
    skos:definition "Term that indicates data sharing of full anonymised data with third party is disallowed"@en ;
    skos:inScheme p7012:privacy-term-classes ;
    skos:prefLabel "Sharing Anonymised Data with 3rd Party Disallowed"@en .

p7012:SharingDataDisallowed a rdfs:Class,
        skos:Concept,
        dpv:Prohibition,
        p7012:DataSharingTerm ;
    dct:created "2024-12-17"^^xsd:date ;
    rdfs:isDefinedBy p7012: ;
    sw:term_status "accepted"@en ;
    skos:broader dpv:Prohibition,
        p7012:DataSharingTerm ;
    skos:definition "Term that indicates Data Sharing is not allowed"@en ;
    skos:inScheme p7012:privacy-term-classes ;
    skos:prefLabel "Sharing Data Disallowed"@en .

p7012:SharingDataNonAnonymised3PDisallowed a rdfs:Class,
        skos:Concept,
        dpv:Prohibition,
        p7012:DataSharingTerm ;
    dct:created "2024-12-17"^^xsd:date ;
    rdfs:isDefinedBy p7012: ;
    sw:term_status "accepted"@en ;
    skos:broader p7012:SharingDataDisallowed ;
    skos:definition "Term that indicates data sharing of non-anonymised data with third party is disallowed"@en ;
    skos:inScheme p7012:privacy-term-classes ;
    skos:prefLabel "Sharing Non-Anonymised Data with 3rd Party Disallowed"@en .

p7012:SharingDataNonAnonymisedDisallowed a rdfs:Class,
        skos:Concept,
        dpv:Prohibition,
        p7012:DataSharingTerm ;
    dct:created "2024-12-17"^^xsd:date ;
    rdfs:isDefinedBy p7012: ;
    sw:term_status "accepted"@en ;
    skos:broader p7012:SharingDataDisallowed ;
    skos:definition "Term that indicates Data Sharing for fully anonymised data is not allowed"@en ;
    skos:inScheme p7012:privacy-term-classes ;
    skos:prefLabel "Sharing Non-Anonymised Data Disallowed"@en .

p7012:ThirdParty a rdfs:Class,
        skos:Concept ;
    dct:created "2024-12-17"^^xsd:date ;
    rdfs:isDefinedBy p7012: ;
    rdfs:subClassOf dpv:LegalEntity ;
    sw:term_status "accepted"@en ;
    skos:broader dpv:LegalEntity ;
    skos:definition "A party other than the Person and Entity as first and second parties respectively in the contractual interaction"@en ;
    skos:inScheme p7012:entities-classes ;
    skos:prefLabel "Third Party"@en .

p7012:Tracking2PAllowed a rdfs:Class,
        skos:Concept,
        dpv:Permission,
        p7012:TrackingTerm ;
    dct:created "2024-12-17"^^xsd:date ;
    rdfs:isDefinedBy p7012: ;
    sw:term_status "accepted"@en ;
    skos:broader p7012:TrackingAllowed ;
    skos:definition "Term that indicates Tracking 2nd Party is allowed"@en ;
    skos:inScheme p7012:privacy-term-classes ;
    skos:prefLabel "Tracking by 2nd Party Allowed"@en .

p7012:Tracking3PDisallowed a rdfs:Class,
        skos:Concept,
        dpv:Prohibition,
        p7012:TrackingTerm ;
    dct:created "2024-12-17"^^xsd:date ;
    rdfs:isDefinedBy p7012: ;
    sw:term_status "accepted"@en ;
    skos:broader p7012:TrackingDisallowed ;
    skos:definition "Term that indicates Tracking 3rd Party is disallowed"@en ;
    skos:inScheme p7012:privacy-term-classes ;
    skos:prefLabel "Tracking by 3rd Party Disallowed"@en .

p7012:TrackingAllowed a rdfs:Class,
        skos:Concept,
        dpv:Permission,
        p7012:TrackingTerm ;
    dct:created "2024-12-17"^^xsd:date ;
    rdfs:isDefinedBy p7012: ;
    sw:term_status "accepted"@en ;
    skos:broader dpv:Permission,
        p7012:TrackingTerm ;
    skos:definition "Term that indicates Tracking by 2nd and 3rd parties is allowed"@en ;
    skos:inScheme p7012:privacy-term-classes ;
    skos:prefLabel "Tracking Allowed"@en .

p7012:TrackingDisallowed a rdfs:Class,
        skos:Concept,
        dpv:Prohibition,
        p7012:TrackingTerm ;
    dct:created "2024-12-17"^^xsd:date ;
    rdfs:isDefinedBy p7012: ;
    sw:term_status "accepted"@en ;
    skos:broader dpv:Prohibition,
        p7012:TrackingTerm ;
    skos:definition "Term that indicates Tracking by 2nd and 3rd parties is disallowed"@en ;
    skos:inScheme p7012:privacy-term-classes ;
    skos:prefLabel "Tracking Disallowed"@en .

p7012:TrackingTerm a rdfs:Class,
        skos:Concept ;
    dct:created "2024-12-17"^^xsd:date ;
    rdfs:isDefinedBy p7012: ;
    rdfs:subClassOf dpv:ContractualClause ;
    sw:term_status "accepted"@en ;
    skos:broader dpv:ContractualClause ;
    skos:definition "Term related to Tracking"@en ;
    skos:inScheme p7012:privacy-term-classes ;
    skos:prefLabel "Tracking Term"@en .

p7012:TrackingWithFPDisallowed a rdfs:Class,
        skos:Concept,
        dpv:Prohibition,
        p7012:TrackingTerm ;
    dct:created "2024-12-17"^^xsd:date ;
    rdfs:isDefinedBy p7012: ;
    sw:term_status "accepted"@en ;
    skos:broader p7012:TrackingDisallowed ;
    skos:definition "Term that indicates Tracking involving use of Fingerprinting is not allowed"@en ;
    skos:inScheme p7012:privacy-term-classes ;
    skos:prefLabel "Tracking With FP Disallowed"@en .

p7012:TrackingWithPIIDisallowed a rdfs:Class,
        skos:Concept,
        dpv:Prohibition,
        p7012:TrackingTerm ;
    dct:created "2024-12-17"^^xsd:date ;
    rdfs:isDefinedBy p7012: ;
    sw:term_status "accepted"@en ;
    skos:broader p7012:TrackingDisallowed ;
    skos:definition "Term that indicates Tracking involving use of PII is not allowed"@en ;
    skos:inScheme p7012:privacy-term-classes ;
    skos:prefLabel "Tracking With PII Disallowed"@en .

p7012:TrackingWithoutFPAllowed a rdfs:Class,
        skos:Concept,
        dpv:Permission,
        p7012:TrackingTerm ;
    dct:created "2024-12-17"^^xsd:date ;
    rdfs:isDefinedBy p7012: ;
    sw:term_status "accepted"@en ;
    skos:broader p7012:TrackingAllowed ;
    skos:definition "Term that indicates Tracking is allowed but only if it does not involve Fingerprinting"@en ;
    skos:inScheme p7012:privacy-term-classes ;
    skos:prefLabel "Tracking Without FP Allowed"@en .

p7012:TrackingWithoutPIIAllowed a rdfs:Class,
        skos:Concept,
        dpv:Permission,
        p7012:TrackingTerm ;
    dct:created "2024-12-17"^^xsd:date ;
    rdfs:isDefinedBy p7012: ;
    sw:term_status "accepted"@en ;
    skos:broader p7012:TrackingAllowed ;
    skos:definition "Term that indicates Tracking is allowed but only if it does not use any PII"@en ;
    skos:inScheme p7012:privacy-term-classes ;
    skos:prefLabel "Tracking Without PII Allowed"@en .

p7012:TransparencyExAnte a rdfs:Class,
        skos:Concept,
        dpv:Obligation,
        p7012:TransparencyTerm ;
    dct:created "2024-12-17"^^xsd:date ;
    rdfs:isDefinedBy p7012: ;
    sw:term_status "accepted"@en ;
    skos:broader p7012:TransparencyRequired ;
    skos:definition "Term that indicates transparency is obligated ahead of intended process i.e. ex-ante transparency"@en ;
    skos:inScheme p7012:privacy-term-classes ;
    skos:prefLabel "Transparency Ex Ante"@en .

p7012:TransparencyExPost a rdfs:Class,
        skos:Concept,
        dpv:Obligation,
        p7012:TransparencyTerm ;
    dct:created "2024-12-17"^^xsd:date ;
    rdfs:isDefinedBy p7012: ;
    sw:term_status "accepted"@en ;
    skos:broader p7012:TransparencyRequired ;
    skos:definition "Term that indicates transparency is obligated after intended process i.e. ex-post transparency"@en ;
    skos:inScheme p7012:privacy-term-classes ;
    skos:prefLabel "Transparency Ex Post"@en .

p7012:TransparencyNotRequired a rdfs:Class,
        skos:Concept,
        p7012:TransparencyTerm ;
    dct:created "2024-12-17"^^xsd:date ;
    rdfs:isDefinedBy p7012: ;
    sw:term_status "accepted"@en ;
    skos:broader p7012:TransparencyRequired ;
    skos:definition "Term that indicates transparency is not required to be provided"@en ;
    skos:inScheme p7012:privacy-term-classes ;
    skos:prefLabel "Transparency Not Required"@en .

p7012:TransparencyOnRequest a rdfs:Class,
        skos:Concept,
        dpv:Obligation,
        p7012:TransparencyTerm ;
    dct:created "2024-12-17"^^xsd:date ;
    rdfs:isDefinedBy p7012: ;
    sw:term_status "accepted"@en ;
    skos:broader p7012:TransparencyRequired ;
    skos:definition "Term that indicates transparency is obligated upon request"@en ;
    skos:inScheme p7012:privacy-term-classes ;
    skos:prefLabel "Transparency On Request"@en .

p7012:TransparencyRequired a rdfs:Class,
        skos:Concept,
        dpv:Obligation,
        p7012:TransparencyTerm ;
    dct:created "2024-12-17"^^xsd:date ;
    rdfs:isDefinedBy p7012: ;
    sw:term_status "accepted"@en ;
    skos:broader dpv:Obligation,
        p7012:TransparencyTerm ;
    skos:definition "Term that indicates transparency is obligated"@en ;
    skos:inScheme p7012:privacy-term-classes ;
    skos:prefLabel "Transparency Required"@en .

p7012:TransparencyTerm a rdfs:Class,
        skos:Concept ;
    dct:created "2024-12-17"^^xsd:date ;
    rdfs:isDefinedBy p7012: ;
    rdfs:subClassOf dpv:ContractualClause ;
    sw:term_status "accepted"@en ;
    skos:broader dpv:ContractualClause ;
    skos:definition "Term that indicates transparency as an obligation"@en ;
    skos:inScheme p7012:privacy-term-classes ;
    skos:prefLabel "Transparency Term"@en .

<https://w3id.org/dpv/standards/p7012> a owl:Ontology,
        profile:Profile ;
    dct:bibliographicCitation "Harshvardhan J. Pandit, Beatriz Esteves, Georg P. Krog, Paul Ryan, Delaram Golpayegani, Julian Flake (2025) Data Privacy Vocabulary (DPV) – Version 2.0. In: Demartini, G., et al. The Semantic Web – ISWC 2024. ISWC 2024. Lecture Notes in Computer Science, vol 15233. Springer, Cham. https://doi.org/10.1007/978-3-031-77847-6_10" ;
    dct:conformsTo "http://www.w3.org/2000/01/rdf-schema",
        "http://www.w3.org/2004/02/skos/core" ;
    dct:created "2025-01-12"@en ;
    dct:creator [ a dct:Agent,
                foaf:Person ;
            org:memberOf [ a foaf:Organization ;
                    foaf:name "JLINC Labs" ] ;
            foaf:name "Iain Henderson" ],
        [ a dct:Agent,
                foaf:Person ;
            scoro:hasORCID "0000-0002-5068-3714" ;
            org:memberOf [ a foaf:Organization ;
                    foaf:name "ADAPT Centre, Dublin City University" ] ;
            foaf:homepage "https://harshp.com/" ;
            foaf:name "Harshvardhan J. Pandit" ],
        [ a dct:Agent,
                foaf:Person ;
            scoro:hasORCID "0000-0003-0259-7560" ;
            org:memberOf [ a foaf:Organization ;
                    foaf:name "IDLab, IMEC, Ghent University" ] ;
            foaf:name "Beatriz Esteves" ] ;
    dct:description "Extension to the Data Privacy Vocabulary (DPV) providing concepts for implementing IEEE P7012"@en ;
    dct:identifier "https://w3id.org/dpv/standards/p7012" ;
    dct:issued "2025-01-12"@en ;
    dct:license <https://www.w3.org/copyright/document-license-2023/> ;
    dct:modified "2025-03-16"@en ;
    dct:publisher <https://www.w3.org/> ;
    dct:source <https://www.w3.org/groups/cg/dpvcg/> ;
    dct:title "Extension for IEEE P7012"@en ;
    bibo:doi "10.5281/zenodo.12505841" ;
    bibo:status "http://purl.org/ontology/bibo/status/draft" ;
    vann:preferredNamespacePrefix "p7012" ;
    vann:preferredNamespaceUri "https://w3id.org/dpv/standards/p7012#" ;
    rdfs:Label "P7012"@en ;
    owl:versionIRI <https://w3id.org/dpv/2.1/standards/p7012> ;
    owl:versionInfo "2.1" ;
    profile:hasResource <https://w3id.org/dpv/examples>,
        <https://w3id.org/dpv/guides>,
        <https://w3id.org/dpv/primer>,
        p7012:serialisation-html,
        p7012:serialisation-jsonld,
        p7012:serialisation-n3,
        p7012:serialisation-rdf,
        p7012:serialisation-ttl ;
    profile:isProfileOf rdfs:,
        skos:,
        <https://w3id.org/dpv> ;
    foaf:logo <https://w3id.org/dpv/media/logo.png> ;
    schema:version "2.1" .

p7012:hasAgent a rdf:Property,
        skos:Concept ;
    dcam:rangeIncludes p7012:Agent ;
    dct:created "2024-12-17"^^xsd:date ;
    rdfs:isDefinedBy p7012: ;
    rdfs:subPropertyOf dpv:hasEntity ;
    sw:term_status "accepted"@en ;
    skos:broader dpv:hasEntity ;
    skos:definition "Specifies the agent that represents a party and can act on behalf"@en ;
    skos:inScheme p7012:entities-properties ;
    skos:prefLabel "has agent"@en ;
    schema:rangeIncludes p7012:Agent .

p7012:hasAgentBehaviour a rdf:Property,
        skos:Concept ;
    dcam:rangeIncludes p7012:AgentBehaviour ;
    dct:created "2024-12-17"^^xsd:date ;
    rdfs:isDefinedBy p7012: ;
    sw:term_status "accepted"@en ;
    skos:definition "Relation that indicates the behaviour of Privacy Agents"@en ;
    skos:inScheme p7012:privacy-term-properties ;
    skos:prefLabel "has agent behaviour"@en ;
    schema:rangeIncludes p7012:AgentBehaviour .

p7012:hasAgreement a rdf:Property,
        skos:Concept ;
    dcam:rangeIncludes p7012:Agreement ;
    dct:created "2024-12-17"^^xsd:date ;
    rdfs:isDefinedBy p7012: ;
    sw:term_status "accepted"@en ;
    skos:definition "Indicates the inclusion or applicability of the specified Privacy Term"@en ;
    skos:inScheme p7012:process-properties ;
    skos:prefLabel "has agreement"@en ;
    schema:rangeIncludes p7012:Agreement .

p7012:hasAgreementPreference a rdf:Property,
        skos:Concept ;
    dcam:rangeIncludes p7012:AgreementPreference ;
    dct:created "2024-12-17"^^xsd:date ;
    rdfs:isDefinedBy p7012: ;
    sw:term_status "accepted"@en ;
    skos:definition "Indicates the inclusion or applicability of the specified Privacy Preference"@en ;
    skos:inScheme p7012:process-properties ;
    skos:prefLabel "has privacy preference"@en ;
    schema:rangeIncludes p7012:AgreementPreference .

p7012:hasAgreementRegistry a rdf:Property,
        skos:Concept ;
    dcam:rangeIncludes p7012:AgreementRegistry ;
    dct:created "2024-12-17"^^xsd:date ;
    rdfs:isDefinedBy p7012: ;
    sw:term_status "accepted"@en ;
    skos:definition "Indicates the inclusion or applicability of the specified Privacy Term Registry"@en ;
    skos:inScheme p7012:process-properties ;
    skos:prefLabel "has agreement registry"@en ;
    schema:rangeIncludes p7012:AgreementRegistry .

p7012:hasConflictResolution a rdf:Property,
        skos:Concept ;
    dcam:rangeIncludes p7012:ConflictResolutionTerm ;
    dct:created "2024-12-17"^^xsd:date ;
    rdfs:isDefinedBy p7012: ;
    sw:term_status "accepted"@en ;
    skos:definition "Relation that indicates the Conflict Resolution Term that should be used"@en ;
    skos:inScheme p7012:privacy-term-properties ;
    skos:prefLabel "has conflict resolution"@en ;
    schema:rangeIncludes p7012:ConflictResolutionTerm .

p7012:hasDataSharingTerm a rdf:Property,
        skos:Concept ;
    dcam:rangeIncludes p7012:DataSharingTerm ;
    dct:created "2024-12-17"^^xsd:date ;
    rdfs:isDefinedBy p7012: ;
    sw:term_status "accepted"@en ;
    skos:definition "Relation that associates a Data Sharing Term"@en ;
    skos:inScheme p7012:privacy-term-properties ;
    skos:prefLabel "has data sharing term"@en ;
    schema:rangeIncludes p7012:DataSharingTerm .

p7012:hasDeonticInterpretation a rdf:Property,
        skos:Concept ;
    dcam:rangeIncludes p7012:DeonticInterpretationTerm ;
    dct:created "2024-12-17"^^xsd:date ;
    rdfs:isDefinedBy p7012: ;
    sw:term_status "accepted"@en ;
    skos:definition "Relation that indicates the Deontic Interpretation Term that should be used"@en ;
    skos:inScheme p7012:privacy-term-properties ;
    skos:prefLabel "has deontic interpretation"@en ;
    schema:rangeIncludes p7012:DeonticInterpretationTerm .

p7012:hasFirstParty a rdf:Property,
        skos:Concept ;
    dcam:rangeIncludes p7012:Person ;
    dct:created "2024-12-17"^^xsd:date ;
    rdfs:isDefinedBy p7012: ;
    rdfs:subPropertyOf dpv:hasEntity ;
    sw:term_status "accepted"@en ;
    skos:broader dpv:hasEntity ;
    skos:definition "Specifies the human individual or Person involved as the first party"@en ;
    skos:inScheme p7012:entities-properties ;
    skos:prefLabel "has first party"@en ;
    schema:rangeIncludes p7012:Person .

p7012:hasHumanReadableFormat a rdf:Property,
        skos:Concept ;
    dcam:rangeIncludes xsd:anyURI ;
    dct:created "2024-12-17"^^xsd:date ;
    rdfs:isDefinedBy p7012: ;
    sw:term_status "accepted"@en ;
    skos:definition "Indicates the specified resource is a human readable format of the subject"@en ;
    skos:inScheme p7012:process-properties ;
    skos:prefLabel "has human readable format"@en ;
    schema:rangeIncludes xsd:anyURI .

p7012:hasMachineReadableFormat a rdf:Property,
        skos:Concept ;
    dcam:rangeIncludes xsd:anyURI ;
    dct:created "2024-12-17"^^xsd:date ;
    rdfs:isDefinedBy p7012: ;
    sw:term_status "accepted"@en ;
    skos:definition "Indicates the specified resource is a machine readable format of the subject"@en ;
    skos:inScheme p7012:process-properties ;
    skos:prefLabel "has machine readable format"@en ;
    skos:scopeNote "To assist in interpreting the resource, we strongly suggest using dct:conformsTo with an appropriate URI to indicate the specific standard or specification used to express the resource"@en ;
    schema:rangeIncludes xsd:anyURI .

p7012:hasP7012Endpoint a rdf:Property,
        skos:Concept ;
    dcam:rangeIncludes p7012:P7012Endpoint ;
    dct:created "2024-12-17"^^xsd:date ;
    rdfs:isDefinedBy p7012: ;
    sw:term_status "accepted"@en ;
    skos:definition "Indicates the endpoint, such as a URL or an address, where P7012 related communications and interactions can be made"@en ;
    skos:inScheme p7012:process-properties ;
    skos:prefLabel "has P7012 endpoint"@en ;
    schema:rangeIncludes p7012:P7012Endpoint .

p7012:hasParty a rdf:Property,
        skos:Concept ;
    dcam:rangeIncludes p7012:Party ;
    dct:created "2024-12-17"^^xsd:date ;
    rdfs:isDefinedBy p7012: ;
    rdfs:subPropertyOf dpv:hasEntity ;
    sw:term_status "accepted"@en ;
    skos:broader dpv:hasEntity ;
    skos:definition "Specifies that an entity is a party to the context i.e. it has decision making abilities or has obligations and responsibilities"@en ;
    skos:inScheme p7012:entities-properties ;
    skos:prefLabel "has party"@en ;
    schema:rangeIncludes p7012:Party .

p7012:hasPortabilityTerm a rdf:Property,
        skos:Concept ;
    dcam:rangeIncludes p7012:PortabilityTerm ;
    dct:created "2024-12-17"^^xsd:date ;
    rdfs:isDefinedBy p7012: ;
    sw:term_status "accepted"@en ;
    skos:definition "Relation that associates a Portability Term"@en ;
    skos:inScheme p7012:privacy-term-properties ;
    skos:prefLabel "has portability term"@en ;
    schema:rangeIncludes p7012:PortabilityTerm .

p7012:hasPreferenceApplicability a rdf:Property,
        skos:Concept ;
    dcam:rangeIncludes p7012:PreferenceApplicability ;
    dct:created "2024-12-17"^^xsd:date ;
    rdfs:isDefinedBy p7012: ;
    sw:term_status "accepted"@en ;
    skos:definition "Relation that indicates the applicability of Privacy Preference(s)"@en ;
    skos:inScheme p7012:privacy-term-properties ;
    skos:prefLabel "has preference applicability"@en ;
    schema:rangeIncludes p7012:PreferenceApplicability .

p7012:hasProfilingTerm a rdf:Property,
        skos:Concept ;
    dcam:rangeIncludes p7012:ProfilingTerm ;
    dct:created "2024-12-17"^^xsd:date ;
    rdfs:isDefinedBy p7012: ;
    sw:term_status "accepted"@en ;
    skos:definition "Relation that associates a Profiling Term"@en ;
    skos:inScheme p7012:privacy-term-properties ;
    skos:prefLabel "has profiling term"@en ;
    schema:rangeIncludes p7012:ProfilingTerm .

p7012:hasSecondParty a rdf:Property,
        skos:Concept ;
    dcam:rangeIncludes p7012:Entity ;
    dct:created "2024-12-17"^^xsd:date ;
    rdfs:isDefinedBy p7012: ;
    rdfs:subPropertyOf dpv:hasEntity ;
    sw:term_status "accepted"@en ;
    skos:broader dpv:hasEntity ;
    skos:definition "Specifies the entity organisation involved as the second party"@en ;
    skos:inScheme p7012:entities-properties ;
    skos:prefLabel "has second party"@en ;
    schema:rangeIncludes p7012:Entity .

p7012:hasThirdParty a rdf:Property,
        skos:Concept ;
    dcam:rangeIncludes p7012:ThirdParty ;
    dct:created "2024-12-17"^^xsd:date ;
    rdfs:isDefinedBy p7012: ;
    rdfs:subPropertyOf dpv:hasThirdParty ;
    sw:term_status "accepted"@en ;
    skos:broader dpv:hasThirdParty ;
    skos:definition "Specifies the a party other than the person or Entity that is involved"@en ;
    skos:inScheme p7012:entities-properties ;
    skos:prefLabel "has third party"@en ;
    schema:rangeIncludes p7012:ThirdParty .

p7012:hasTrackingTerm a rdf:Property,
        skos:Concept ;
    dcam:rangeIncludes p7012:TrackingTerm ;
    dct:created "2024-12-17"^^xsd:date ;
    rdfs:isDefinedBy p7012: ;
    sw:term_status "accepted"@en ;
    skos:definition "Relation that associates a Tracking Term"@en ;
    skos:inScheme p7012:privacy-term-properties ;
    skos:prefLabel "has tracking term"@en ;
    schema:rangeIncludes p7012:TrackingTerm .

p7012:hasTransparencyTerm a rdf:Property,
        skos:Concept ;
    dcam:rangeIncludes p7012:TransparencyTerm ;
    dct:created "2024-12-17"^^xsd:date ;
    rdfs:isDefinedBy p7012: ;
    sw:term_status "accepted"@en ;
    skos:definition "Relation that associates a Transparency Term"@en ;
    skos:inScheme p7012:privacy-term-properties ;
    skos:prefLabel "has transparency term"@en ;
    schema:rangeIncludes p7012:TransparencyTerm .

p7012:serialisation-html a profile:ResourceDescriptor ;
    dct:conformsTo <https://www.w3.org/TR/html/> ;
    dct:format <https://www.iana.org/assignments/media-types/text/html> ;
    dct:title "Extension for IEEE P7012 - HTML serialiation" ;
    profile:hasArtifact <https://w3id.org/dpv/standards/p7012/p7012.html> ;
    profile:hasRole role:specification .

p7012:serialisation-jsonld a profile:ResourceDescriptor ;
    dct:conformsTo <https://www.w3.org/TR/json-ld11/> ;
    dct:format <https://www.iana.org/assignments/media-types/application/ld+json> ;
    dct:title "Extension for IEEE P7012 - JSON-LD serialiation" ;
    profile:hasArtifact <https://w3id.org/dpv/standards/p7012/p7012.jsonld> ;
    profile:hasRole role:vocabulary .

p7012:serialisation-n3 a profile:ResourceDescriptor ;
    dct:conformsTo <https://www.w3.org/TeamSubmission/n3/> ;
    dct:format <https://www.iana.org/assignments/media-types/text/n3> ;
    dct:title "Extension for IEEE P7012 - N3 serialiation" ;
    profile:hasArtifact <https://w3id.org/dpv/standards/p7012/p7012.n3> ;
    profile:hasRole role:vocabulary .

p7012:serialisation-rdf a profile:ResourceDescriptor ;
    dct:conformsTo rdf: ;
    dct:format <https://www.iana.org/assignments/media-types/application/rdf+xml> ;
    dct:title "Extension for IEEE P7012 - RDF/XML serialiation" ;
    profile:hasArtifact <https://w3id.org/dpv/standards/p7012/p7012.rdf> ;
    profile:hasRole role:vocabulary .

p7012:serialisation-ttl a profile:ResourceDescriptor ;
    dct:conformsTo <https://www.w3.org/TR/turtle/> ;
    dct:format <https://www.iana.org/assignments/media-types/text/turtle> ;
    dct:title "Extension for IEEE P7012 - Turtle serialiation" ;
    profile:hasArtifact <https://w3id.org/dpv/standards/p7012/p7012.ttl> ;
    profile:hasRole role:vocabulary .

<https://w3id.org/dpv/examples> a profile:ResourceDescriptor ;
    dct:conformsTo <https://www.w3.org/TR/html/> ;
    dct:format <https://www.iana.org/assignments/media-types/text/html> ;
    dct:title "Examples for Data Privacy Vocabulary" ;
    profile:hasArtifact <https://w3id.org/dpv/examples> ;
    profile:hasRole role:guidance .

<https://w3id.org/dpv/guides> a profile:ResourceDescriptor ;
    dct:conformsTo <https://www.w3.org/TR/html/> ;
    dct:format <https://www.iana.org/assignments/media-types/text/html> ;
    dct:title "Guides for Data Privacy Vocabulary" ;
    profile:hasArtifact <https://w3id.org/dpv/guides> ;
    profile:hasRole role:guidance .

<https://w3id.org/dpv/primer> a profile:ResourceDescriptor ;
    dct:conformsTo <https://www.w3.org/TR/html/> ;
    dct:format <https://www.iana.org/assignments/media-types/text/html> ;
    dct:title "Primer for Data Privacy Vocabulary" ;
    profile:hasArtifact <https://w3id.org/dpv/primer> ;
    profile:hasRole role:guidance .

p7012:purpose-classes a skos:ConceptScheme .

p7012:data-classes a skos:ConceptScheme .

p7012:entities-properties a skos:ConceptScheme .

p7012:entities-classes a skos:ConceptScheme .

p7012:process-properties a skos:ConceptScheme .

p7012:process-classes a skos:ConceptScheme .

p7012:privacy-term-properties a skos:ConceptScheme .

p7012:agreement-classes a skos:ConceptScheme .

p7012:status-classes a skos:ConceptScheme .

p7012:privacy-term-classes a skos:ConceptScheme .

