@prefix bibo: <http://purl.org/ontology/bibo/> .
@prefix dcam: <http://purl.org/dc/dcam/> .
@prefix dcat: <http://www.w3.org/ns/dcat#> .
@prefix dct: <http://purl.org/dc/terms/> .
@prefix dex-owl: <https://w3id.org/dpv/examples/owl#> .
@prefix dpv-owl: <https://w3id.org/dpv/owl#> .
@prefix foaf: <http://xmlns.com/foaf/0.1/> .
@prefix odrl: <http://www.w3.org/ns/odrl/2/> .
@prefix owl: <http://www.w3.org/2002/07/owl#> .
@prefix profile: <http://www.w3.org/ns/dx/prof/> .
@prefix rdf: <http://www.w3.org/1999/02/22-rdf-syntax-ns#> .
@prefix rdfs: <http://www.w3.org/2000/01/rdf-schema#> .
@prefix role: <http://www.w3.org/ns/dx/prof/role/> .
@prefix schema: <https://schema.org/> .
@prefix skos: <http://www.w3.org/2004/02/skos/core#> .
@prefix spl: <https://specialprivacy.ercim.eu/langs/usage-policy#> .
@prefix svd: <https://specialprivacy.ercim.eu/vocabs/data#> .
@prefix svpr: <https://specialprivacy.ercim.eu/vocabs/processing#> .
@prefix svpu: <https://specialprivacy.ercim.eu/vocabs/purposes#> .
@prefix sw: <http://www.w3.org/2003/06/sw-vocab-status/ns#> .
@prefix vann: <http://purl.org/vocab/vann/> .
@prefix xsd: <http://www.w3.org/2001/XMLSchema#> .

dcat:Resource a rdfs:Class,
        owl:Class ;
    dct:created "2022-11-02"^^xsd:date ;
    rdfs:isDefinedBy dpv-owl: ;
    skos:prefLabel "dcat:Resource"@en ;
    skos:scopeNote "A dataset, data service, or any other resource associated with Right Exercise - such as for providing a copy of data"@en .

dpv-owl:AILiteracy a rdfs:Class,
        owl:Class,
        dpv-owl:OrganisationalMeasure ;
    dct:contributor "Harshvardhan J. Pandit" ;
    dct:created "2024-05-17"^^xsd:date ;
    rdfs:isDefinedBy dpv-owl: ;
    rdfs:subClassOf dpv-owl:DigitalLiteracy ;
    sw:term_status "accepted"@en ;
    skos:definition "Providing skills, knowledge, and understanding to enable reading, writing, analysing, reasoning, and communicating regarding AI"@en ;
    skos:prefLabel "AI Literacy"@en .

dpv-owl:AcademicResearch a rdfs:Class,
        owl:Class,
        dpv-owl:Purpose ;
    dct:contributor "Harshvardhan J. Pandit, Javier Fernández, Axel Polleres, Elmar Kiesling, Fajar Ekaputra, Simon Steyskal" ;
    dct:created "2019-04-05"^^xsd:date ;
    rdfs:isDefinedBy dpv-owl: ;
    rdfs:subClassOf dpv-owl:ResearchAndDevelopment ;
    sw:term_status "accepted"@en ;
    skos:definition "Purposes associated with conducting or assisting with research conducted in an academic context e.g. within universities"@en ;
    skos:prefLabel "Academic Research"@en ;
    skos:related svpu:Education .

dpv-owl:AcademicScientificOrganisation a rdfs:Class,
        owl:Class ;
    dct:contributor "Harshvardhan J. Pandit" ;
    dct:created "2022-02-02"^^xsd:date ;
    dct:modified "2020-10-05"^^xsd:date ;
    dct:source [ a schema:WebPage ;
            schema:name "ADMS controlled vocabulary" ;
            schema:url "http://purl.org/adms" ] ;
    rdfs:isDefinedBy dpv-owl: ;
    rdfs:subClassOf dpv-owl:Organisation ;
    sw:term_status "accepted"@en ;
    skos:definition "Organisations related to academia or scientific pursuits e.g. Universities, Schools, Research Bodies"@en ;
    skos:prefLabel "Academic or Scientific Organisation"@en .

dpv-owl:Access a rdfs:Class,
        owl:Class,
        dpv-owl:Processing ;
    dct:contributor "Harshvardhan J. Pandit, Georg P. Krog" ;
    dct:created "2022-06-15"^^xsd:date ;
    rdfs:isDefinedBy dpv-owl: ;
    rdfs:subClassOf dpv-owl:Use ;
    sw:term_status "accepted"@en ;
    skos:definition "to access data"@en ;
    skos:prefLabel "Access"@en .

dpv-owl:AccessControlMethod a rdfs:Class,
        owl:Class,
        dpv-owl:TechnicalMeasure ;
    dct:contributor "Axel Polleres, Rob Brennan, Harshvardhan J. Pandit, Mark Lizar" ;
    dct:created "2019-04-05"^^xsd:date ;
    vann:example dex-owl:E0020 ;
    rdfs:isDefinedBy dpv-owl: ;
    rdfs:subClassOf dpv-owl:TechnicalMeasure ;
    sw:term_status "accepted"@en ;
    skos:definition "Methods which restrict access to a place or resource"@en ;
    skos:prefLabel "Access Control Method"@en .

dpv-owl:AccountManagement a rdfs:Class,
        owl:Class,
        dpv-owl:Purpose ;
    dct:contributor "Georg P. Krog, Harshvardhan J. Pandit, Beatriz Esteves" ;
    dct:created "2021-09-08"^^xsd:date ;
    rdfs:isDefinedBy dpv-owl: ;
    rdfs:subClassOf dpv-owl:Purpose ;
    sw:term_status "accepted"@en ;
    skos:definition "Account Management refers to purposes associated with account management, such as to create, provide, maintain, and manage accounts"@en ;
    skos:prefLabel "Account Management"@en .

dpv-owl:Acquire a rdfs:Class,
        owl:Class,
        dpv-owl:Processing ;
    dct:created "2019-05-07"^^xsd:date ;
    dct:source [ a schema:WebPage ;
            schema:name "GDPR Art.4-2" ;
            schema:url "https://eur-lex.europa.eu/eli/reg/2016/679/art_4/par_2/oj" ] ;
    rdfs:isDefinedBy dpv-owl: ;
    rdfs:subClassOf dpv-owl:Obtain ;
    sw:term_status "accepted"@en ;
    skos:definition "to come into possession or control of the data"@en ;
    skos:prefLabel "Acquire"@en .

dpv-owl:ActiveRight a rdfs:Class,
        owl:Class,
        dpv-owl:Right ;
    dct:contributor "Harshvardhan J. Pandit, Beatriz Esteves, Georg P. Krog, Paul Ryan" ;
    dct:created "2022-10-22"^^xsd:date ;
    rdfs:isDefinedBy dpv-owl: ;
    rdfs:subClassOf dpv-owl:Right ;
    sw:term_status "accepted"@en ;
    skos:definition "The right(s) applicable, provided, or expected that need to be (actively) exercised"@en ;
    skos:prefLabel "Active Right"@en ;
    skos:scopeNote "Active rights require the entity to expressly exercise them. For example, a Data Subject exercising their right to withdraw their consent."@en .

dpv-owl:ActivelyInvolved a rdfs:Class,
        owl:Class,
        dpv-owl:InvolvementStatus ;
    dct:contributor "Harshvardhan J. Pandit, Delaram Golpayegani, Georg P. Krog, Paul Ryan" ;
    dct:created "2024-05-10"^^xsd:date ;
    rdfs:isDefinedBy dpv-owl: ;
    rdfs:subClassOf dpv-owl:InvolvementStatus ;
    sw:term_status "accepted"@en ;
    skos:definition "Status indicating the specified context is 'actively' involved"@en ;
    skos:prefLabel "Actively Involved"@en ;
    skos:scopeNote "An example of active involvement is a person directly using a system to enter information"@en .

dpv-owl:ActivityCompleted a rdfs:Class,
        owl:Class,
        dpv-owl:ActivityStatus ;
    dct:contributor "Harshvardhan J. Pandit" ;
    dct:created "2022-05-18"^^xsd:date ;
    rdfs:isDefinedBy dpv-owl: ;
    rdfs:subClassOf dpv-owl:ActivityStatus ;
    sw:term_status "accepted"@en ;
    skos:definition "State of an activity that has completed i.e. is fully in the past"@en ;
    skos:prefLabel "Activity Completed"@en .

dpv-owl:ActivityHalted a rdfs:Class,
        owl:Class,
        dpv-owl:ActivityStatus ;
    dct:contributor "Harshvardhan J. Pandit" ;
    dct:created "2022-05-18"^^xsd:date ;
    rdfs:isDefinedBy dpv-owl: ;
    rdfs:subClassOf dpv-owl:ActivityStatus ;
    sw:term_status "accepted"@en ;
    skos:definition "State of an activity that was occuring in the past, and has been halted or paused or stopped"@en ;
    skos:prefLabel "Activity Halted"@en .

dpv-owl:ActivityMonitoring a rdfs:Class,
        owl:Class,
        dpv-owl:TechnicalMeasure ;
    dct:contributor "Harshvardhan J. Pandit" ;
    dct:created "2022-08-17"^^xsd:date ;
    dct:source [ a schema:WebPage ;
            schema:name "ENISA Reference Incident Classification Taxonomy 2018" ;
            schema:url "https://www.enisa.europa.eu/publications/reference-incident-classification-taxonomy/" ] ;
    rdfs:isDefinedBy dpv-owl: ;
    rdfs:subClassOf dpv-owl:TechnicalMeasure ;
    sw:term_status "accepted"@en ;
    skos:definition "Monitoring of activities including assessing whether they have been successfully initiated and completed"@en ;
    skos:prefLabel "Activity Monitoring"@en .

dpv-owl:ActivityNotCompleted a rdfs:Class,
        owl:Class,
        dpv-owl:ActivityStatus ;
    dct:contributor "Harshvardhan J. Pandit" ;
    dct:created "2022-11-30"^^xsd:date ;
    rdfs:isDefinedBy dpv-owl: ;
    rdfs:subClassOf dpv-owl:ActivityStatus ;
    sw:term_status "accepted"@en ;
    skos:definition "State of an activity that could not be completed, but has reached some end state"@en ;
    skos:prefLabel "Activity Not Completed"@en ;
    skos:scopeNote "This relates to a 'Stop' state as distinct from a 'Halt' state. It makes no comments on whether the Activity can be resumed or continued towards completion."@en .

dpv-owl:ActivityOngoing a rdfs:Class,
        owl:Class,
        dpv-owl:ActivityStatus ;
    dct:contributor "Harshvardhan J. Pandit" ;
    dct:created "2022-05-18"^^xsd:date ;
    rdfs:isDefinedBy dpv-owl: ;
    rdfs:subClassOf dpv-owl:ActivityStatus ;
    sw:term_status "accepted"@en ;
    skos:definition "State of an activity occurring in continuation i.e. currently ongoing"@en ;
    skos:prefLabel "Activity Ongoing"@en .

dpv-owl:ActivityPlanned a rdfs:Class,
        owl:Class,
        dpv-owl:ActivityStatus ;
    dct:contributor "Harshvardhan J. Pandit" ;
    dct:created "2024-05-19"^^xsd:date ;
    rdfs:isDefinedBy dpv-owl: ;
    rdfs:subClassOf dpv-owl:ActivityStatus ;
    sw:term_status "accepted"@en ;
    skos:definition "State of an activity being planned with concrete plans for implementation"@en ;
    skos:prefLabel "Activity Planned"@en .

dpv-owl:ActivityProposed a rdfs:Class,
        owl:Class,
        dpv-owl:ActivityStatus ;
    dct:contributor "Harshvardhan J. Pandit" ;
    dct:created "2022-05-18"^^xsd:date ;
    dct:modified "2024-05-19"^^xsd:date ;
    rdfs:isDefinedBy dpv-owl: ;
    rdfs:subClassOf dpv-owl:ActivityStatus ;
    sw:term_status "accepted"@en ;
    skos:definition "State of an activity being proposed without any concrete plans for implementation"@en ;
    skos:prefLabel "Activity Proposed"@en .

dpv-owl:ActivityStatus a rdfs:Class,
        owl:Class ;
    dct:contributor "Harshvardhan J. Pandit" ;
    dct:created "2022-05-18"^^xsd:date ;
    vann:example dex-owl:E0054 ;
    rdfs:isDefinedBy dpv-owl: ;
    rdfs:subClassOf dpv-owl:Status ;
    sw:term_status "accepted"@en ;
    skos:definition "Status associated with activity operations and lifecycles"@en ;
    skos:prefLabel "Activity Status"@en .

dpv-owl:Adapt a rdfs:Class,
        owl:Class,
        dpv-owl:Processing ;
    dct:created "2019-05-07"^^xsd:date ;
    dct:source [ a schema:WebPage ;
            schema:name "GDPR Art.4-2" ;
            schema:url "https://eur-lex.europa.eu/eli/reg/2016/679/art_4/par_2/oj" ] ;
    rdfs:isDefinedBy dpv-owl: ;
    rdfs:subClassOf dpv-owl:Transform ;
    sw:term_status "accepted"@en ;
    skos:definition "to modify the data, often rewritten into a new form for a new use"@en ;
    skos:prefLabel "Adapt"@en .

dpv-owl:Adult a rdfs:Class,
        owl:Class,
        dpv-owl:DataSubject ;
    dct:contributor "Georg P. Krog" ;
    dct:created "2022-03-30"^^xsd:date ;
    rdfs:isDefinedBy dpv-owl: ;
    rdfs:subClassOf dpv-owl:DataSubject ;
    sw:term_status "accepted"@en ;
    skos:definition "A natural person that is not a child i.e. has attained some legally specified age of adulthood"@en ;
    skos:prefLabel "Adult"@en .

dpv-owl:Advertising a rdfs:Class,
        owl:Class,
        dpv-owl:Purpose ;
    dct:contributor "Georg P. Krog, Harshvardhan J. Pandit, Beatriz Esteves" ;
    dct:created "2020-11-04"^^xsd:date ;
    rdfs:isDefinedBy dpv-owl: ;
    rdfs:subClassOf dpv-owl:Marketing ;
    sw:term_status "accepted"@en ;
    skos:definition "Purposes associated with conducting advertising i.e. process or artefact used to call attention to a product, service, etc. through announcements, notices, or other forms of communication"@en ;
    skos:prefLabel "Advertising"@en ;
    skos:scopeNote "Advertising is a subset of Marketing. Advertising by itself does not indicate 'personalisation' i.e. personalised ads."@en .

dpv-owl:AgeVerification a rdfs:Class,
        owl:Class,
        dpv-owl:Purpose ;
    dct:contributor "Beatriz Esteves, Arthit Suriyawongkul, Harshvardhan J. Pandit" ;
    dct:created "2024-02-14"^^xsd:date ;
    rdfs:isDefinedBy dpv-owl: ;
    rdfs:subClassOf dpv-owl:Verification ;
    sw:term_status "accepted"@en ;
    skos:definition "Purposes associated with verifying or authenticating age or age related information as a form of security"@en ;
    skos:prefLabel "Age Verification"@en ;
    skos:scopeNote "Age Verification can include verification of the exact age, e.g. being 21 years old, a date, e.g. birth date is 01 January 1969, or a condition, e.g. age is over 21 years and the person is an adult. Specific dedicated resources should be used to further express information and processes associated with Age Verification, for example the Age Verification Vocabulary https://w3id.org/age/"@en .

dpv-owl:Aggregate a rdfs:Class,
        owl:Class,
        dpv-owl:Processing ;
    dct:contributor "Beatriz Esteves, Harshvardhan J. Pandit" ;
    dct:created "2024-04-14"^^xsd:date ;
    dct:source [ a schema:WebPage ;
            schema:name "SPECIAL Project" ;
            schema:url "https://specialprivacy.ercim.eu/vocabs/processing" ] ;
    rdfs:isDefinedBy dpv-owl: ;
    rdfs:subClassOf dpv-owl:Alter ;
    sw:term_status "accepted"@en ;
    skos:definition "to aggregate data"@en ;
    skos:prefLabel "Aggregate"@en ;
    skos:related svpr:Aggregate .

dpv-owl:AlgorithmicLogic a rdfs:Class,
        owl:Class ;
    dct:contributor "Harshvardhan J. Pandit" ;
    dct:created "2022-01-26"^^xsd:date ;
    dct:modified "2023-12-10"^^xsd:date ;
    rdfs:isDefinedBy dpv-owl: ;
    rdfs:subClassOf dpv-owl:ProcessingContext ;
    sw:term_status "accepted"@en ;
    skos:definition "The algorithmic logic applied or used"@en ;
    skos:prefLabel "Algorithmic Logic"@en ;
    skos:scopeNote "Algorithmic Logic is intended as a broad concept for explaining the use of algorithms and automated decisions making within Processing. To describe the actual algorithm, see the Algorithm concept."@en .

dpv-owl:Align a rdfs:Class,
        owl:Class,
        dpv-owl:Processing ;
    dct:created "2019-05-07"^^xsd:date ;
    dct:source [ a schema:WebPage ;
            schema:name "GDPR Art.4-2" ;
            schema:url "https://eur-lex.europa.eu/eli/reg/2016/679/art_4/par_2/oj" ] ;
    rdfs:isDefinedBy dpv-owl: ;
    rdfs:subClassOf dpv-owl:Transform ;
    sw:term_status "accepted"@en ;
    skos:definition "to adjust the data to be in relation to another data"@en ;
    skos:prefLabel "Align"@en .

dpv-owl:Alter a rdfs:Class,
        owl:Class,
        dpv-owl:Processing ;
    dct:created "2019-05-07"^^xsd:date ;
    dct:source [ a schema:WebPage ;
            schema:name "GDPR Art.4-2" ;
            schema:url "https://eur-lex.europa.eu/eli/reg/2016/679/art_4/par_2/oj" ] ;
    rdfs:isDefinedBy dpv-owl: ;
    rdfs:subClassOf dpv-owl:Transform ;
    sw:term_status "accepted"@en ;
    skos:definition "to change the data without changing it into something else"@en ;
    skos:prefLabel "Alter"@en .

dpv-owl:Analyse a rdfs:Class,
        owl:Class,
        dpv-owl:Processing ;
    dct:created "2019-05-07"^^xsd:date ;
    dct:source [ a schema:WebPage ;
            schema:name "SPECIAL Project" ;
            schema:url "https://specialprivacy.ercim.eu/vocabs/processing" ] ;
    rdfs:isDefinedBy dpv-owl: ;
    rdfs:subClassOf dpv-owl:Use ;
    sw:term_status "accepted"@en ;
    skos:definition "to study or examine the data in detail"@en ;
    skos:prefLabel "Analyse"@en ;
    skos:related svpr:Analyse .

dpv-owl:Anonymisation a rdfs:Class,
        owl:Class,
        dpv-owl:TechnicalMeasure ;
    dct:contributor "Axel Polleres, Rob Brennan, Harshvardhan J. Pandit, Mark Lizar, Maya Borges, Damien Desfontaines" ;
    dct:created "2019-04-05"^^xsd:date ;
    dct:modified "2022-11-24"^^xsd:date ;
    dct:source [ a schema:WebPage ;
            schema:name "ISO 29100:2011" ;
            schema:url "https://www.iso.org/standard/45123.html" ] ;
    rdfs:isDefinedBy dpv-owl: ;
    rdfs:subClassOf dpv-owl:Deidentification ;
    sw:term_status "accepted"@en ;
    skos:definition "Anonymisation is the process by which data is irreversibly altered in such a way that a data subject can no longer be identified directly or indirectly, either by the entity holding the data alone or in collaboration with other entities and information sources"@en ;
    skos:prefLabel "Anonymisation"@en .

dpv-owl:Anonymise a rdfs:Class,
        owl:Class,
        dpv-owl:Processing ;
    dct:created "2019-05-07"^^xsd:date ;
    dct:source [ a schema:WebPage ;
            schema:name "SPECIAL Project" ;
            schema:url "https://specialprivacy.ercim.eu/vocabs/processing" ] ;
    rdfs:isDefinedBy dpv-owl: ;
    rdfs:subClassOf dpv-owl:Transform ;
    sw:term_status "accepted"@en ;
    skos:definition "to irreversibly alter personal data in such a way that an unique data subject can no longer be identified directly or indirectly or in combination with other data"@en ;
    skos:prefLabel "Anonymise"@en ;
    skos:related svpr:Anonymise .

dpv-owl:AnonymisedData a rdfs:Class,
        owl:Class ;
    dct:contributor "Piero Bonatti" ;
    dct:created "2022-01-19"^^xsd:date ;
    rdfs:isDefinedBy dpv-owl: ;
    rdfs:subClassOf dpv-owl:NonPersonalData ;
    sw:term_status "accepted"@en ;
    skos:definition "Personal Data that has been (fully and completely) anonymised so that it is no longer considered Personal Data"@en ;
    skos:prefLabel "Anonymised Data"@en ;
    skos:scopeNote "It is advised to carefully consider indicating data is fully or completely anonymised by determining whether the data by itself or in combination with other data can identify a person. Failing this condition, the data should be denoted as PseudonymisedData. To indicate data is anonymised only for a specified entity (e.g. within an organisation), the concept ContextuallyAnonymisedData (as subclass of PseudonymisedData) should be used instead of AnonymisedData."@en .

dpv-owl:Applicability a rdfs:Class,
        owl:Class ;
    dct:contributor "Harshvardhan J. Pandit" ;
    dct:created "2023-08-24"^^xsd:date ;
    vann:example dex-owl:E0053 ;
    rdfs:isDefinedBy dpv-owl: ;
    rdfs:subClassOf dpv-owl:Context ;
    sw:term_status "accepted"@en ;
    skos:definition "Concept provided to represent indication of cases where the information or context is not applicable (N/A) or not available or this is not known or determined yet. If the information is applicable and available, this concept should not be used."@en ;
    skos:prefLabel "Applicability"@en ;
    skos:scopeNote "These concepts are useful in closed-world interpretations, for example in forms where a field must have a value to explicitly denote it is not applicable or the information is not available yet."@en .

dpv-owl:Applicant a rdfs:Class,
        owl:Class,
        dpv-owl:DataSubject ;
    dct:contributor "Harshvardhan J. Pandit, Georg P. Krog, Julian Flake, Paul Ryan, Beatriz Esteves" ;
    dct:created "2022-04-06"^^xsd:date ;
    rdfs:isDefinedBy dpv-owl: ;
    rdfs:subClassOf dpv-owl:DataSubject ;
    sw:term_status "accepted"@en ;
    skos:definition "Data subjects that are applicants in some context"@en ;
    skos:prefLabel "Applicant"@en .

dpv-owl:Assess a rdfs:Class,
        owl:Class,
        dpv-owl:Processing ;
    dct:contributor "Harshvardhan J. Pandit, Georg P. Krog" ;
    dct:created "2022-06-15"^^xsd:date ;
    rdfs:isDefinedBy dpv-owl: ;
    rdfs:subClassOf dpv-owl:Use ;
    sw:term_status "accepted"@en ;
    skos:definition "to assess data for some criteria"@en ;
    skos:prefLabel "Assess"@en .

dpv-owl:Assessment a rdfs:Class,
        owl:Class,
        dpv-owl:OrganisationalMeasure ;
    dct:contributor "Harshvardhan J. Pandit" ;
    dct:created "2021-09-08"^^xsd:date ;
    rdfs:isDefinedBy dpv-owl: ;
    rdfs:subClassOf dpv-owl:OrganisationalMeasure ;
    sw:term_status "accepted"@en ;
    skos:definition "The document, plan, or process for assessment or determination towards a purpose e.g. assessment of legality or impact assessments"@en ;
    skos:prefLabel "Assessment"@en .

dpv-owl:AssetManagementProcedures a rdfs:Class,
        owl:Class,
        dpv-owl:OrganisationalMeasure ;
    dct:contributor "Harshvardhan J. Pandit" ;
    dct:created "2022-08-17"^^xsd:date ;
    dct:source [ a schema:WebPage ;
            schema:name "ENISA 5G Cybersecurity Standards" ;
            schema:url "https://www.enisa.europa.eu/publications/5g-cybersecurity-standards" ] ;
    rdfs:isDefinedBy dpv-owl: ;
    rdfs:subClassOf dpv-owl:GovernanceProcedures ;
    sw:term_status "accepted"@en ;
    skos:definition "Procedures related to management of assets"@en ;
    skos:prefLabel "Asset Management Procedures"@en .

dpv-owl:AssistiveAutomation a rdfs:Class,
        owl:Class,
        dpv-owl:AutomationLevel ;
    dct:contributor "Harshvardhan J. Pandit, Delaram Golpayegani" ;
    dct:created "2023-12-10"^^xsd:date ;
    dct:modified "2024-04-20"^^xsd:date ;
    dct:source [ a schema:WebPage ;
            schema:name "ISO/IEC 22989:2022 Artificial intelligence concepts and terminology" ;
            schema:url "https://www.iso.org/standard/74296.html" ] ;
    rdfs:isDefinedBy dpv-owl: ;
    rdfs:subClassOf dpv-owl:AutomationLevel ;
    sw:term_status "accepted"@en ;
    skos:definition "Level of automation corresponding to Level 1 in ISO/IEC 22989:2022 where automation is limited to parts of the system or a specific part of the system in a manner that does not change the control of the human in using/driving the system"@en ;
    skos:prefLabel "Assistive Automation"@en ;
    skos:scopeNote "Human Involvement is implied here, specifically the ability to make decisions regarding operations, but also possibly for intervention, oversight, and verification"@en .

dpv-owl:AsylumSeeker a rdfs:Class,
        owl:Class,
        dpv-owl:DataSubject ;
    dct:contributor "Georg P. Krog" ;
    dct:created "2022-06-15"^^xsd:date ;
    rdfs:isDefinedBy dpv-owl: ;
    rdfs:subClassOf dpv-owl:VulnerableDataSubject ;
    sw:term_status "accepted"@en ;
    skos:definition "Data subjects that are asylum seekers"@en ;
    skos:prefLabel "Asylum Seeker"@en .

dpv-owl:AsymmetricCryptography a rdfs:Class,
        owl:Class,
        dpv-owl:TechnicalMeasure ;
    dct:contributor "Harshvardhan J. Pandit" ;
    dct:created "2022-08-17"^^xsd:date ;
    dct:source [ a schema:WebPage ;
            schema:name "ENISA Reference Incident Classification Taxonomy 2018" ;
            schema:url "https://www.enisa.europa.eu/publications/reference-incident-classification-taxonomy/" ] ;
    rdfs:isDefinedBy dpv-owl: ;
    rdfs:subClassOf dpv-owl:CryptographicMethods ;
    sw:term_status "accepted"@en ;
    skos:definition "Use of public-key cryptography or asymmetric cryptography involving a public and private pair of keys"@en ;
    skos:prefLabel "Asymmetric Cryptography"@en .

dpv-owl:AsymmetricEncryption a rdfs:Class,
        owl:Class,
        dpv-owl:TechnicalMeasure ;
    dct:contributor "Harshvardhan J. Pandit" ;
    dct:created "2022-08-17"^^xsd:date ;
    dct:source [ a schema:WebPage ;
            schema:name "ENISA Data Pseudonymisation: Advanced Techniques and Use Cases" ;
            schema:url "https://www.enisa.europa.eu/publications/data-pseudonymisation-advanced-techniques-and-use-cases" ] ;
    rdfs:isDefinedBy dpv-owl: ;
    rdfs:subClassOf dpv-owl:Encryption ;
    sw:term_status "accepted"@en ;
    skos:definition "Use of asymmetric cryptography to encrypt data"@en ;
    skos:prefLabel "Asymmetric Encryption"@en .

dpv-owl:AuditApproved a rdfs:Class,
        owl:Class,
        dpv-owl:AuditStatus ;
    dct:contributor "Harshvardhan J. Pandit" ;
    dct:created "2022-05-18"^^xsd:date ;
    rdfs:isDefinedBy dpv-owl: ;
    rdfs:subClassOf dpv-owl:AuditStatus ;
    sw:term_status "accepted"@en ;
    skos:definition "State of being approved through the audit"@en ;
    skos:prefLabel "Audit Approved"@en .

dpv-owl:AuditConditionallyApproved a rdfs:Class,
        owl:Class,
        dpv-owl:AuditStatus ;
    dct:contributor "Paul Ryan" ;
    dct:created "2022-06-29"^^xsd:date ;
    rdfs:isDefinedBy dpv-owl: ;
    rdfs:subClassOf dpv-owl:AuditStatus ;
    sw:term_status "accepted"@en ;
    skos:definition "State of being conditionally approved through the audit"@en ;
    skos:prefLabel "Audit Conditionally Approved"@en ;
    skos:scopeNote "A \"conditional approval\" is intended to reflect states where the audit has identified further changes which must be implemented before considering the audit has been 'passed', without requiring another audit to validate them. This is distinct from the case where an audit has state 'rejected', which means changes must be made and submitted for review. The requirements of a 'conditional acceptance' are expected to be minor or not significant enough to warrant another audit to review them."@en .

dpv-owl:AuditNotRequired a rdfs:Class,
        owl:Class,
        dpv-owl:AuditStatus ;
    dct:contributor "Harshvardhan J. Pandit" ;
    dct:created "2022-05-18"^^xsd:date ;
    rdfs:isDefinedBy dpv-owl: ;
    rdfs:subClassOf dpv-owl:AuditStatus ;
    sw:term_status "accepted"@en ;
    skos:definition "State where an audit is determined as not being required"@en ;
    skos:prefLabel "Audit Not Required"@en .

dpv-owl:AuditRejected a rdfs:Class,
        owl:Class,
        dpv-owl:AuditStatus ;
    dct:contributor "Harshvardhan J. Pandit" ;
    dct:created "2022-05-18"^^xsd:date ;
    rdfs:isDefinedBy dpv-owl: ;
    rdfs:subClassOf dpv-owl:AuditStatus ;
    sw:term_status "accepted"@en ;
    skos:definition "State of not being approved or being rejected through the audit"@en ;
    skos:prefLabel "Audit Rejected"@en .

dpv-owl:AuditRequested a rdfs:Class,
        owl:Class,
        dpv-owl:AuditStatus ;
    dct:contributor "Harshvardhan J. Pandit" ;
    dct:created "2022-05-18"^^xsd:date ;
    rdfs:isDefinedBy dpv-owl: ;
    rdfs:subClassOf dpv-owl:AuditStatus ;
    sw:term_status "accepted"@en ;
    skos:definition "State of an audit being requested whose outcome is not yet known"@en ;
    skos:prefLabel "Audit Requested"@en .

dpv-owl:AuditRequired a rdfs:Class,
        owl:Class,
        dpv-owl:AuditStatus ;
    dct:contributor "Harshvardhan J. Pandit" ;
    dct:created "2022-05-18"^^xsd:date ;
    rdfs:isDefinedBy dpv-owl: ;
    rdfs:subClassOf dpv-owl:AuditStatus ;
    sw:term_status "accepted"@en ;
    skos:definition "State where an audit is determined as being required but has not been conducted"@en ;
    skos:prefLabel "Audit Required"@en .

dpv-owl:AuditStatus a rdfs:Class,
        owl:Class ;
    dct:contributor "Harshvardhan J. Pandit" ;
    dct:created "2022-05-18"^^xsd:date ;
    vann:example dex-owl:E0056,
        dex-owl:E0057 ;
    rdfs:isDefinedBy dpv-owl: ;
    rdfs:subClassOf dpv-owl:Status ;
    sw:term_status "accepted"@en ;
    skos:definition "Status associated with Auditing or Investigation"@en ;
    skos:prefLabel "Audit Status"@en .

dpv-owl:Authentication-ABC a rdfs:Class,
        owl:Class,
        dpv-owl:TechnicalMeasure ;
    dct:contributor "Harshvardhan J. Pandit" ;
    dct:created "2022-08-17"^^xsd:date ;
    dct:source [ a schema:WebPage ;
            schema:name "ENISA Data Protection Engineering" ;
            schema:url "https://www.enisa.europa.eu/publications/data-protection-engineering" ] ;
    rdfs:isDefinedBy dpv-owl: ;
    rdfs:subClassOf dpv-owl:CryptographicAuthentication ;
    sw:term_status "accepted"@en ;
    skos:definition "Use of Attribute Based Credentials (ABC) to perform and manage authentication"@en ;
    skos:prefLabel "Authentication using ABC"@en .

dpv-owl:Authentication-PABC a rdfs:Class,
        owl:Class,
        dpv-owl:TechnicalMeasure ;
    dct:contributor "Harshvardhan J. Pandit" ;
    dct:created "2022-08-17"^^xsd:date ;
    dct:source [ a schema:WebPage ;
            schema:name "ENISA Data Protection Engineering" ;
            schema:url "https://www.enisa.europa.eu/publications/data-protection-engineering" ] ;
    rdfs:isDefinedBy dpv-owl: ;
    rdfs:subClassOf dpv-owl:CryptographicAuthentication ;
    sw:term_status "accepted"@en ;
    skos:definition "Use of Privacy-enhancing Attribute Based Credentials (ABC) to perform and manage authentication"@en ;
    skos:prefLabel "Authentication using PABC"@en .

dpv-owl:AuthenticationProtocols a rdfs:Class,
        owl:Class,
        dpv-owl:TechnicalMeasure ;
    dct:contributor "Axel Polleres, Rob Brennan, Harshvardhan J. Pandit, Mark Lizar" ;
    dct:created "2019-04-05"^^xsd:date ;
    rdfs:isDefinedBy dpv-owl: ;
    rdfs:subClassOf dpv-owl:TechnicalMeasure ;
    sw:term_status "accepted"@en ;
    skos:definition "Protocols involving validation of identity i.e. authentication of a person or information"@en ;
    skos:prefLabel "Authentication Protocols"@en .

dpv-owl:AuthorisationProcedure a rdfs:Class,
        owl:Class,
        dpv-owl:OrganisationalMeasure ;
    dct:contributor "Axel Polleres, Rob Brennan, Harshvardhan J. Pandit, Mark Lizar" ;
    dct:created "2019-04-05"^^xsd:date ;
    rdfs:isDefinedBy dpv-owl: ;
    rdfs:subClassOf dpv-owl:SecurityProcedure ;
    sw:term_status "accepted"@en ;
    skos:definition "Procedures for determining authorisation through permission or authority"@en ;
    skos:prefLabel "Authorisation Procedure"@en ;
    skos:scopeNote "non-technical authorisation procedures: How is it described on an organisational level, who gets access to the data"@en .

dpv-owl:AuthorisationProtocols a rdfs:Class,
        owl:Class,
        dpv-owl:TechnicalMeasure ;
    dct:contributor "Harshvardhan J. Pandit" ;
    dct:created "2022-08-17"^^xsd:date ;
    dct:source [ a schema:WebPage ;
            schema:name "ENISA Reference Incident Classification Taxonomy 2018" ;
            schema:url "https://www.enisa.europa.eu/publications/reference-incident-classification-taxonomy/" ] ;
    rdfs:isDefinedBy dpv-owl: ;
    rdfs:subClassOf dpv-owl:TechnicalMeasure ;
    sw:term_status "accepted"@en ;
    skos:definition "Protocols involving authorisation of roles or profiles to determine permission, rights, or privileges"@en ;
    skos:prefLabel "Authorisation Protocols"@en .

dpv-owl:Authority a rdfs:Class,
        owl:Class ;
    dct:contributor "Georg P. Krog, Paul Ryan, Harshvardhan J. Pandit" ;
    dct:created "2020-11-04"^^xsd:date ;
    rdfs:isDefinedBy dpv-owl: ;
    rdfs:subClassOf dpv-owl:GovernmentalOrganisation ;
    sw:term_status "accepted"@en ;
    skos:definition "An authority with the power to create or enforce laws, or determine their compliance."@en ;
    skos:prefLabel "Authority"@en .

dpv-owl:AuthorityInformed a rdfs:Class,
        owl:Class,
        dpv-owl:EntityInformedStatus ;
    dct:contributor "Harshvardhan J. Pandit, Delaram Golpayegani, Georg P. Krog, Paul Ryan" ;
    dct:created "2024-05-10"^^xsd:date ;
    rdfs:isDefinedBy dpv-owl: ;
    rdfs:subClassOf dpv-owl:EntityInformed ;
    sw:term_status "accepted"@en ;
    skos:definition "Status indicating Authority has been informed about the specified context"@en ;
    skos:prefLabel "Authority Informed"@en .

dpv-owl:AuthorityUninformed a rdfs:Class,
        owl:Class,
        dpv-owl:EntityInformedStatus ;
    dct:contributor "Harshvardhan J. Pandit, Delaram Golpayegani, Georg P. Krog, Paul Ryan" ;
    dct:created "2024-05-10"^^xsd:date ;
    rdfs:isDefinedBy dpv-owl: ;
    rdfs:subClassOf dpv-owl:EntityUninformed ;
    sw:term_status "accepted"@en ;
    skos:definition "Status indicating Authority is uninformed i.e. has not been informed about the specified context"@en ;
    skos:prefLabel "Authority Uninformed"@en .

dpv-owl:AutomatedDecisionMaking a rdfs:Class,
        owl:Class ;
    dct:contributor "Harshvardhan J. Pandit, Piero Bonatti" ;
    dct:created "2020-11-04"^^xsd:date ;
    dct:modified "2022-09-07"^^xsd:date ;
    dct:source [ a schema:WebPage ;
            schema:name "GDPR Art.4-2" ;
            schema:url "https://eur-lex.europa.eu/eli/reg/2016/679/art_4/par_2/oj" ] ;
    rdfs:isDefinedBy dpv-owl: ;
    rdfs:subClassOf dpv-owl:DecisionMaking ;
    sw:term_status "accepted"@en ;
    skos:definition "Processing that involves automated decision making"@en ;
    skos:prefLabel "Automated Decision Making"@en ;
    skos:scopeNote "Automated decision making can be defined as “the ability to make decisions by technological means without human involvement.” (“Guidelines on Automated individual decision-making and Profiling for the purposes of Regulation 2016/679 (wp251rev.01)”, 2018, p. 8)"@en .

dpv-owl:AutomatedScoringOfIndividuals a rdfs:Class,
        owl:Class,
        dpv-owl:ScoringOfIndividuals ;
    dct:contributor "Harshvardhan J. Pandit" ;
    dct:created "2024-04-14"^^xsd:date ;
    rdfs:isDefinedBy dpv-owl: ;
    rdfs:subClassOf dpv-owl:ScoringOfIndividuals ;
    sw:term_status "accepted"@en ;
    skos:definition "Processing that involves automated scoring of individuals"@en ;
    skos:prefLabel "Automated Scoring of Individuals"@en ;
    skos:scopeNote "Scoring can lead to the action being considered Decision Making if the scoring is itself a decision - see 2023-MAR-16 opinion of Advocate General on Case C 634/21. Therefore, the assessment of whether scoring was automated or not is important given the legal obligations surrounding automated decision making e.g. in GDPR"@en .

dpv-owl:AutomationLevel a rdfs:Class,
        owl:Class ;
    dct:contributor "Harshvardhan J. Pandit, Delaram Golpayegani" ;
    dct:created "2023-12-10"^^xsd:date ;
    dct:modified "2024-04-20"^^xsd:date ;
    dct:source [ a schema:WebPage ;
            schema:name "ISO/IEC 22989:2022 Artificial intelligence concepts and terminology" ;
            schema:url "https://www.iso.org/standard/74296.html" ] ;
    vann:example dex-owl:E0013 ;
    rdfs:isDefinedBy dpv-owl: ;
    rdfs:subClassOf dpv-owl:ProcessingContext ;
    sw:term_status "accepted"@en ;
    skos:definition "Indication of degree or level of automation associated with specified context"@en ;
    skos:prefLabel "Automation Level"@en ;
    skos:scopeNote "This concept was called 'Automation' in previous versions"@en .

dpv-owl:Autonomous a rdfs:Class,
        owl:Class,
        dpv-owl:AutomationLevel ;
    dct:contributor "Harshvardhan J. Pandit, Delaram Golpayegani" ;
    dct:created "2023-12-10"^^xsd:date ;
    dct:modified "2024-04-20"^^xsd:date ;
    dct:source [ a schema:WebPage ;
            schema:name "ISO/IEC 22989:2022 Artificial intelligence concepts and terminology" ;
            schema:url "https://www.iso.org/standard/74296.html" ] ;
    rdfs:isDefinedBy dpv-owl: ;
    rdfs:subClassOf dpv-owl:AutomationLevel ;
    sw:term_status "accepted"@en ;
    skos:definition "Level of automation corresponding to Level 6 in ISO/IEC 22989:2022 where the automation in system is capable of modifying its operation domain or its goals without external intervention, control or oversight"@en ;
    skos:prefLabel "Autonomous"@en ;
    skos:scopeNote "Though Autonomous, such operations can still be associated with dpv:HumanInvolved e.g. for inputs, oversight or verification"@en .

dpv-owl:BackgroundChecks a rdfs:Class,
        owl:Class,
        dpv-owl:OrganisationalMeasure ;
    dct:contributor "Harshvardhan J. Pandit" ;
    dct:created "2022-08-17"^^xsd:date ;
    dct:source [ a schema:WebPage ;
            schema:name "ENISA 5G Cybersecurity Standards" ;
            schema:url "https://www.enisa.europa.eu/publications/5g-cybersecurity-standards" ] ;
    rdfs:isDefinedBy dpv-owl: ;
    rdfs:subClassOf dpv-owl:SecurityProcedure ;
    sw:term_status "accepted"@en ;
    skos:definition "Procedure where the background of an entity is assessed to identity vulnerabilities and threats due to their current or intended role"@en ;
    skos:prefLabel "Background Checks"@en .

dpv-owl:BiometricAuthentication a rdfs:Class,
        owl:Class,
        dpv-owl:TechnicalMeasure ;
    dct:contributor "Harshvardhan J. Pandit" ;
    dct:created "2022-08-17"^^xsd:date ;
    dct:source [ a schema:WebPage ;
            schema:name "ENISA Reference Incident Classification Taxonomy 2018" ;
            schema:url "https://www.enisa.europa.eu/publications/reference-incident-classification-taxonomy/" ] ;
    rdfs:isDefinedBy dpv-owl: ;
    rdfs:subClassOf dpv-owl:AuthenticationProtocols ;
    sw:term_status "accepted"@en ;
    skos:definition "Use of biometric data for authentication"@en ;
    skos:prefLabel "Biometric Authentication"@en .

dpv-owl:CannotChallengeProcess a rdfs:Class,
        owl:Class,
        dpv-owl:EntityNonPermissiveInvolvement ;
    dct:contributor "Harshvardhan J. Pandit, Delaram Golpayegani, Steve Hickman" ;
    dct:created "2024-05-11"^^xsd:date ;
    rdfs:isDefinedBy dpv-owl: ;
    rdfs:subClassOf dpv-owl:EntityNonPermissiveInvolvement ;
    sw:term_status "accepted"@en ;
    skos:definition "Involvement where entity cannot challenge the process of specified context"@en ;
    skos:prefLabel "Cannot Challenge Process"@en ;
    skos:scopeNote "Challenge refers to raising questions about validity, necessity, correctness, or other similar 'trustworthiness' attributes regarding the process or plan or implementation"@en .

dpv-owl:CannotChallengeProcessInput a rdfs:Class,
        owl:Class,
        dpv-owl:EntityNonPermissiveInvolvement ;
    dct:contributor "Harshvardhan J. Pandit, Delaram Golpayegani, Steve Hickman" ;
    dct:created "2024-05-11"^^xsd:date ;
    rdfs:isDefinedBy dpv-owl: ;
    rdfs:subClassOf dpv-owl:EntityNonPermissiveInvolvement ;
    sw:term_status "accepted"@en ;
    skos:definition "Involvement where entity cannot challenge input of specified context"@en ;
    skos:prefLabel "Cannot Challenge Process Input"@en .

dpv-owl:CannotChallengeProcessOutput a rdfs:Class,
        owl:Class,
        dpv-owl:EntityNonPermissiveInvolvement ;
    dct:contributor "Harshvardhan J. Pandit, Delaram Golpayegani, Steve Hickman" ;
    dct:created "2024-05-11"^^xsd:date ;
    rdfs:isDefinedBy dpv-owl: ;
    rdfs:subClassOf dpv-owl:EntityNonPermissiveInvolvement ;
    sw:term_status "accepted"@en ;
    skos:definition "Involvement where entity cannot challenge the output of specified context"@en ;
    skos:prefLabel "Cannot Challenge Process Output"@en ;
    skos:scopeNote "Challenge refers to raising questions about validity, necessity, correctness, or other similar 'trustworthiness' attributes regarding the output of the process or plan or implementation (where output is distinct from the process itself)"@en .

dpv-owl:CannotCorrectProcess a rdfs:Class,
        owl:Class,
        dpv-owl:EntityNonPermissiveInvolvement ;
    dct:contributor "Harshvardhan J. Pandit, Delaram Golpayegani, Steve Hickman" ;
    dct:created "2024-05-11"^^xsd:date ;
    rdfs:isDefinedBy dpv-owl: ;
    rdfs:subClassOf dpv-owl:EntityNonPermissiveInvolvement ;
    sw:term_status "accepted"@en ;
    skos:definition "Involvement where entity cannot correct the process of specified context"@en ;
    skos:prefLabel "Cannot Correct Process"@en .

dpv-owl:CannotCorrectProcessInput a rdfs:Class,
        owl:Class,
        dpv-owl:EntityNonPermissiveInvolvement ;
    dct:contributor "Harshvardhan J. Pandit, Delaram Golpayegani, Steve Hickman" ;
    dct:created "2024-05-11"^^xsd:date ;
    rdfs:isDefinedBy dpv-owl: ;
    rdfs:subClassOf dpv-owl:EntityNonPermissiveInvolvement ;
    sw:term_status "accepted"@en ;
    skos:definition "Involvement where entity cannot correct input of specified context"@en ;
    skos:prefLabel "Cannot Correct Process Input"@en .

dpv-owl:CannotCorrectProcessOutput a rdfs:Class,
        owl:Class,
        dpv-owl:EntityNonPermissiveInvolvement ;
    dct:contributor "Harshvardhan J. Pandit, Delaram Golpayegani, Steve Hickman" ;
    dct:created "2024-05-11"^^xsd:date ;
    rdfs:isDefinedBy dpv-owl: ;
    rdfs:subClassOf dpv-owl:EntityNonPermissiveInvolvement ;
    sw:term_status "accepted"@en ;
    skos:definition "Involvement where entity cannot correct the output of specified context"@en ;
    skos:prefLabel "Cannot Correct Process Output"@en .

dpv-owl:CannotObjectToProcess a rdfs:Class,
        owl:Class,
        dpv-owl:EntityNonPermissiveInvolvement ;
    dct:contributor "Harshvardhan J. Pandit, Delaram Golpayegani, Steve Hickman" ;
    dct:created "2024-05-11"^^xsd:date ;
    rdfs:isDefinedBy dpv-owl: ;
    rdfs:subClassOf dpv-owl:EntityNonPermissiveInvolvement ;
    sw:term_status "accepted"@en ;
    skos:definition "Involvement where entity cannot object to process of specified context"@en ;
    skos:prefLabel "Cannot Object to Process"@en .

dpv-owl:CannotOptInToProcess a rdfs:Class,
        owl:Class,
        dpv-owl:EntityNonPermissiveInvolvement ;
    dct:contributor "Harshvardhan J. Pandit, Delaram Golpayegani, Steve Hickman" ;
    dct:created "2024-05-11"^^xsd:date ;
    rdfs:isDefinedBy dpv-owl: ;
    rdfs:subClassOf dpv-owl:EntityNonPermissiveInvolvement ;
    sw:term_status "accepted"@en ;
    skos:definition "Involvement where entity cannot opt-in to specified context"@en ;
    skos:prefLabel "Cannot Opt-in to Process"@en .

dpv-owl:CannotOptOutFromProcess a rdfs:Class,
        owl:Class,
        dpv-owl:EntityNonPermissiveInvolvement ;
    dct:contributor "Harshvardhan J. Pandit, Delaram Golpayegani, Steve Hickman" ;
    dct:created "2024-05-11"^^xsd:date ;
    rdfs:isDefinedBy dpv-owl: ;
    rdfs:subClassOf dpv-owl:EntityNonPermissiveInvolvement ;
    sw:term_status "accepted"@en ;
    skos:definition "Involvement where entity cannot opt-out from specified context"@en ;
    skos:prefLabel "Cannot Opt-out from Process"@en .

dpv-owl:CannotReverseProcessEffects a rdfs:Class,
        owl:Class,
        dpv-owl:EntityNonPermissiveInvolvement ;
    dct:contributor "Harshvardhan J. Pandit, Delaram Golpayegani, Steve Hickman" ;
    dct:created "2024-05-11"^^xsd:date ;
    rdfs:isDefinedBy dpv-owl: ;
    rdfs:subClassOf dpv-owl:EntityNonPermissiveInvolvement ;
    sw:term_status "accepted"@en ;
    skos:definition "Involvement where entity cannot reverse effects of specified context"@en ;
    skos:prefLabel "Cannot Reverse Process Effects"@en ;
    skos:scopeNote "Effects refer to consequences and impacts arising from the process or from the outputs of a process"@en .

dpv-owl:CannotReverseProcessInput a rdfs:Class,
        owl:Class,
        dpv-owl:EntityNonPermissiveInvolvement ;
    dct:contributor "Harshvardhan J. Pandit, Delaram Golpayegani, Steve Hickman" ;
    dct:created "2024-05-11"^^xsd:date ;
    rdfs:isDefinedBy dpv-owl: ;
    rdfs:subClassOf dpv-owl:EntityNonPermissiveInvolvement ;
    sw:term_status "accepted"@en ;
    skos:definition "Involvement where entity cannot reverse input of specified context"@en ;
    skos:prefLabel "Cannot Reverse Process Input"@en ;
    skos:scopeNote "Reversion can be considered a form of correction in some instances. We welcome inputs to further explore and define this relation between correction and reversion concepts."@en .

dpv-owl:CannotReverseProcessOutput a rdfs:Class,
        owl:Class,
        dpv-owl:EntityNonPermissiveInvolvement ;
    dct:contributor "Harshvardhan J. Pandit, Delaram Golpayegani, Steve Hickman" ;
    dct:created "2024-05-11"^^xsd:date ;
    rdfs:isDefinedBy dpv-owl: ;
    rdfs:subClassOf dpv-owl:EntityNonPermissiveInvolvement ;
    sw:term_status "accepted"@en ;
    skos:definition "Involvement where entity cannot reverse output of specified context"@en ;
    skos:prefLabel "Cannot Reverse Process Output"@en .

dpv-owl:CannotWithdrawFromProcess a rdfs:Class,
        owl:Class,
        dpv-owl:EntityNonPermissiveInvolvement ;
    dct:contributor "Harshvardhan J. Pandit, Delaram Golpayegani, Steve Hickman" ;
    dct:created "2024-05-11"^^xsd:date ;
    rdfs:isDefinedBy dpv-owl: ;
    rdfs:subClassOf dpv-owl:EntityNonPermissiveInvolvement ;
    sw:term_status "accepted"@en ;
    skos:definition "Involvement where entity cannot withdraw a previously given assent from specified context"@en ;
    skos:prefLabel "Cannot Withdraw from Process"@en .

dpv-owl:Certification a rdfs:Class,
        owl:Class,
        dpv-owl:OrganisationalMeasure ;
    dct:contributor "Axel Polleres, Rob Brennan, Harshvardhan J. Pandit, Mark Lizar" ;
    dct:created "2019-04-05"^^xsd:date ;
    rdfs:isDefinedBy dpv-owl: ;
    rdfs:subClassOf dpv-owl:CertificationSeal ;
    sw:term_status "accepted"@en ;
    skos:definition "Certification mechanisms, seals, and marks for the purpose of demonstrating compliance"@en ;
    skos:prefLabel "Certification"@en .

dpv-owl:CertificationSeal a rdfs:Class,
        owl:Class,
        dpv-owl:OrganisationalMeasure ;
    dct:contributor "Axel Polleres, Rob Brennan, Harshvardhan J. Pandit, Mark Lizar" ;
    dct:created "2019-04-05"^^xsd:date ;
    rdfs:isDefinedBy dpv-owl: ;
    rdfs:subClassOf dpv-owl:OrganisationalMeasure ;
    sw:term_status "accepted"@en ;
    skos:definition "Certifications, seals, and marks indicating compliance to regulations or practices"@en ;
    skos:prefLabel "Certification and Seal"@en .

dpv-owl:ChallengingProcess a rdfs:Class,
        owl:Class,
        dpv-owl:EntityPermissiveInvolvement ;
    dct:contributor "Harshvardhan J. Pandit, Delaram Golpayegani, Steve Hickman" ;
    dct:created "2024-05-11"^^xsd:date ;
    rdfs:isDefinedBy dpv-owl: ;
    rdfs:subClassOf dpv-owl:EntityPermissiveInvolvement ;
    sw:term_status "accepted"@en ;
    skos:definition "Involvement where entity can challenge the process of specified context"@en ;
    skos:prefLabel "Challenging Process"@en ;
    skos:scopeNote "Challenge refers to raising questions about validity, necessity, correctness, or other similar 'trustworthiness' attributes regarding the process or plan or implementation"@en .

dpv-owl:ChallengingProcessInput a rdfs:Class,
        owl:Class,
        dpv-owl:EntityPermissiveInvolvement ;
    dct:contributor "Harshvardhan J. Pandit, Delaram Golpayegani, Steve Hickman" ;
    dct:created "2024-05-11"^^xsd:date ;
    rdfs:isDefinedBy dpv-owl: ;
    rdfs:subClassOf dpv-owl:EntityPermissiveInvolvement ;
    sw:term_status "accepted"@en ;
    skos:definition "Involvement where entity can challenge input of specified context"@en ;
    skos:prefLabel "Challenging Process Input"@en .

dpv-owl:ChallengingProcessOutput a rdfs:Class,
        owl:Class,
        dpv-owl:EntityPermissiveInvolvement ;
    dct:contributor "Harshvardhan J. Pandit, Delaram Golpayegani, Steve Hickman" ;
    dct:created "2024-05-11"^^xsd:date ;
    rdfs:isDefinedBy dpv-owl: ;
    rdfs:subClassOf dpv-owl:EntityPermissiveInvolvement ;
    sw:term_status "accepted"@en ;
    skos:definition "Involvement where entity can challenge the output of specified context"@en ;
    skos:prefLabel "Challenging Process Output"@en ;
    skos:scopeNote "Challenge refers to raising questions about validity, necessity, correctness, or other similar 'trustworthiness' attributes regarding the output of the process or plan or implementation (where output is distinct from the process itself)"@en .

dpv-owl:Child a rdfs:Class,
        owl:Class,
        dpv-owl:DataSubject ;
    dct:contributor "Harshvardhan J. Pandit" ;
    dct:created "2020-11-25"^^xsd:date ;
    dct:modified "2022-06-22"^^xsd:date ;
    rdfs:isDefinedBy dpv-owl: ;
    rdfs:subClassOf dpv-owl:DataSubject ;
    sw:term_status "accepted"@en ;
    skos:definition "A 'child' is a natural legal person who is below a certain legal age depending on the legal jurisdiction."@en ;
    skos:prefLabel "Child"@en ;
    skos:scopeNote "The legality of age defining a child varies by jurisdiction. In addition, 'child' is distinct from a 'minor'. For example, the legal age for consumption of alcohol can be 21, which makes a person of age 20 a 'minor' in this context. In other cases, 'minor' and 'child' are used interchangeably to refer to a person below some legally defined age."@en .

dpv-owl:Citizen a rdfs:Class,
        owl:Class,
        dpv-owl:DataSubject ;
    dct:contributor "Harshvardhan J. Pandit, Georg P. Krog, Julian Flake, Paul Ryan, Beatriz Esteves" ;
    dct:created "2022-04-06"^^xsd:date ;
    rdfs:isDefinedBy dpv-owl: ;
    rdfs:subClassOf dpv-owl:DataSubject ;
    sw:term_status "accepted"@en ;
    skos:definition "Data subjects that are citizens (for a jurisdiction)"@en ;
    skos:prefLabel "Citizen"@en .

dpv-owl:City a rdfs:Class,
        owl:Class ;
    dct:contributor "Harshvardhan J. Pandit" ;
    dct:created "2022-10-22"^^xsd:date ;
    rdfs:isDefinedBy dpv-owl: ;
    rdfs:subClassOf dpv-owl:Region ;
    sw:term_status "accepted"@en ;
    skos:definition "A region consisting of urban population and commerce"@en ;
    skos:prefLabel "City"@en .

dpv-owl:Client a rdfs:Class,
        owl:Class,
        dpv-owl:DataSubject ;
    dct:contributor "Harshvardhan J. Pandit, Georg P. Krog, Julian Flake, Paul Ryan, Beatriz Esteves" ;
    dct:created "2022-04-06"^^xsd:date ;
    rdfs:isDefinedBy dpv-owl: ;
    rdfs:subClassOf dpv-owl:Customer ;
    sw:term_status "accepted"@en ;
    skos:definition "Data subjects that are clients or recipients of services"@en ;
    skos:prefLabel "Client"@en .

dpv-owl:CloudLocation a rdfs:Class,
        owl:Class,
        dpv-owl:Location ;
    dct:contributor "Harshvardhan J. Pandit" ;
    dct:created "2022-06-15"^^xsd:date ;
    dct:modified "2020-10-05"^^xsd:date ;
    rdfs:isDefinedBy dpv-owl: ;
    rdfs:subClassOf dpv-owl:RemoteLocation ;
    sw:term_status "accepted"@en ;
    skos:definition "Location that is in the 'cloud' i.e. a logical location operated over the internet"@en ;
    skos:prefLabel "Cloud Location"@en .

dpv-owl:CodeOfConduct a rdfs:Class,
        owl:Class,
        dpv-owl:OrganisationalMeasure ;
    dct:contributor "Axel Polleres, Rob Brennan, Harshvardhan J. Pandit, Mark Lizar" ;
    dct:created "2019-04-05"^^xsd:date ;
    rdfs:isDefinedBy dpv-owl: ;
    rdfs:subClassOf dpv-owl:GuidelinesPrinciple ;
    sw:term_status "accepted"@en ;
    skos:definition "A set of rules or procedures outlining the norms and practices for conducting activities"@en ;
    skos:prefLabel "Code of Conduct"@en .

dpv-owl:Collect a rdfs:Class,
        owl:Class,
        dpv-owl:Processing ;
    dct:created "2019-05-07"^^xsd:date ;
    dct:source [ a schema:WebPage ;
            schema:name "GDPR Art.4-2" ;
            schema:url "https://eur-lex.europa.eu/eli/reg/2016/679/art_4/par_2/oj" ],
        [ a schema:WebPage ;
            schema:name "SPECIAL Project" ;
            schema:url "https://specialprivacy.ercim.eu/vocabs/processing" ] ;
    rdfs:isDefinedBy dpv-owl: ;
    rdfs:subClassOf dpv-owl:Obtain ;
    sw:term_status "accepted"@en ;
    skos:definition "to gather data from someone"@en ;
    skos:prefLabel "Collect"@en ;
    skos:related svpr:Collect .

dpv-owl:CollectedData a rdfs:Class,
        owl:Class ;
    dct:created "2023-12-10"^^xsd:date ;
    rdfs:isDefinedBy dpv-owl: ;
    rdfs:subClassOf dpv-owl:Data ;
    sw:term_status "accepted"@en ;
    skos:definition "Data that has been obtained by collecting it from a source"@en ;
    skos:prefLabel "Collected Data"@en .

dpv-owl:CollectedPersonalData a rdfs:Class,
        owl:Class ;
    dct:contributor "Harshvardhan J. Pandit" ;
    dct:created "2022-03-30"^^xsd:date ;
    dct:modified "2023-12-10"^^xsd:date ;
    vann:example dex-owl:E0046 ;
    rdfs:isDefinedBy dpv-owl: ;
    rdfs:subClassOf dpv-owl:CollectedData,
        dpv-owl:PersonalData ;
    sw:term_status "accepted"@en ;
    skos:definition "Personal Data that has been collected from another source such as the Data Subject"@en ;
    skos:prefLabel "Collected Personal Data"@en ;
    skos:scopeNote "To indicate the source of data, use the DataSource concept with the hasDataSource relation"@en .

dpv-owl:CombatClimateChange a rdfs:Class,
        owl:Class,
        dpv-owl:Purpose ;
    dct:contributor "Beatriz Esteves, Harshvardhan J. Pandit" ;
    dct:created "2024-02-14"^^xsd:date ;
    dct:source "DGA 2.16"@en ;
    rdfs:isDefinedBy dpv-owl: ;
    rdfs:subClassOf dpv-owl:PublicBenefit ;
    sw:term_status "accepted"@en ;
    skos:definition "Purposes associated with combating the causes and consequences of climate change, including reducing gas emissions and fighting emergencies such as floods or wildfires"@en ;
    skos:prefLabel "Combat Climate Change"@en .

dpv-owl:Combine a rdfs:Class,
        owl:Class,
        dpv-owl:Processing ;
    dct:created "2019-05-07"^^xsd:date ;
    dct:source [ a schema:WebPage ;
            schema:name "SPECIAL Project" ;
            schema:url "https://specialprivacy.ercim.eu/vocabs/processing" ],
        [ a schema:WebPage ;
            schema:name "GDPR Art.4-2" ;
            schema:url "https://eur-lex.europa.eu/eli/reg/2016/679/art_4/par_2/oj" ] ;
    rdfs:isDefinedBy dpv-owl: ;
    rdfs:subClassOf dpv-owl:Transform ;
    sw:term_status "accepted"@en ;
    skos:definition "to join or merge data"@en ;
    skos:prefLabel "Combine"@en ;
    skos:related svpr:Aggregate .

dpv-owl:CommercialPurpose a rdfs:Class,
        owl:Class,
        dpv-owl:Purpose ;
    dct:contributor "Beatriz Esteves, Harshvardhan J. Pandit" ;
    dct:created "2024-02-14"^^xsd:date ;
    dct:source "DGA 4.4"@en ;
    rdfs:isDefinedBy dpv-owl: ;
    rdfs:subClassOf dpv-owl:Purpose ;
    sw:term_status "accepted"@en ;
    skos:definition "Purposes associated with processing activities performed in a commercial setting or with intention to commercialise"@en ;
    skos:prefLabel "Commercial Purpose"@en .

dpv-owl:CommercialResearch a rdfs:Class,
        owl:Class,
        dpv-owl:Purpose ;
    dct:contributor "Harshvardhan J. Pandit, Javier Fernández, Axel Polleres, Elmar Kiesling, Fajar Ekaputra, Simon Steyskal" ;
    dct:created "2019-04-05"^^xsd:date ;
    dct:modified "2024-04-14"^^xsd:date ;
    rdfs:isDefinedBy dpv-owl: ;
    rdfs:subClassOf dpv-owl:CommercialPurpose,
        dpv-owl:ResearchAndDevelopment ;
    sw:term_status "accepted"@en ;
    skos:definition "Purposes associated with conducting research in a commercial setting or with intention to commercialise e.g. in a company or sponsored by a company"@en ;
    skos:prefLabel "Commercial Research"@en ;
    skos:related svpu:Develop .

dpv-owl:CommerciallyConfidentialData a rdfs:Class,
        owl:Class ;
    dct:created "2024-02-14"^^xsd:date ;
    dct:source "DGA 6.5(c)"@en ;
    rdfs:isDefinedBy dpv-owl: ;
    rdfs:subClassOf dpv-owl:Data ;
    sw:term_status "accepted"@en ;
    skos:definition "Data protected through Commercial Confidentiality Agreements"@en ;
    skos:prefLabel "Commercially Confidential Data"@en .

dpv-owl:CommunicationForCustomerCare a rdfs:Class,
        owl:Class,
        dpv-owl:Purpose ;
    dct:contributor "Georg P. Krog, Harshvardhan J. Pandit, Beatriz Esteves" ;
    dct:created "2020-11-04"^^xsd:date ;
    rdfs:isDefinedBy dpv-owl: ;
    rdfs:subClassOf dpv-owl:CommunicationManagement,
        dpv-owl:CustomerCare ;
    sw:term_status "accepted"@en ;
    skos:definition "Customer Care Communication refers to purposes associated with communicating with customers for assisting them, resolving issues, ensuring satisfaction, etc. in relation to services provided"@en ;
    skos:prefLabel "Communication for Customer Care"@en .

dpv-owl:CommunicationManagement a rdfs:Class,
        owl:Class,
        dpv-owl:Purpose ;
    dct:contributor "Georg P. Krog, Paul Ryan, David Hickey, Harshvardhan J. Pandit" ;
    dct:created "2021-09-01"^^xsd:date ;
    rdfs:isDefinedBy dpv-owl: ;
    rdfs:subClassOf dpv-owl:Purpose ;
    sw:term_status "accepted"@en ;
    skos:definition "Communication Management refers to purposes associated with providing or managing communication activities e.g. to send an email for notifying some information"@en ;
    skos:prefLabel "Communication Management"@en ;
    skos:scopeNote "This purpose by itself does not sufficiently and clearly indicate what the communication is about. As such, it is recommended to combine it with another purpose to indicate the application. For example, Communication of Payment."@en .

dpv-owl:ComplianceAssessment a rdfs:Class,
        owl:Class,
        dpv-owl:OrganisationalMeasure ;
    dct:contributor "Harshvardhan J. Pandit, Georg P. Krog" ;
    dct:created "2024-04-14"^^xsd:date ;
    rdfs:isDefinedBy dpv-owl: ;
    rdfs:subClassOf dpv-owl:Assessment ;
    sw:term_status "accepted"@en ;
    skos:definition "Assessment regarding compliance (e.g. internal policy, regulations)"@en ;
    skos:prefLabel "Compliance Assessment"@en .

dpv-owl:ComplianceIndeterminate a rdfs:Class,
        owl:Class,
        dpv-owl:ComplianceStatus ;
    dct:contributor "Harshvardhan J. Pandit" ;
    dct:created "2022-09-07"^^xsd:date ;
    rdfs:isDefinedBy dpv-owl: ;
    rdfs:subClassOf dpv-owl:ComplianceStatus ;
    sw:term_status "accepted"@en ;
    skos:definition "State where the status of compliance has not been fully assessed, evaluated, or determined"@en ;
    skos:prefLabel "Compliance Indeterminate"@en .

dpv-owl:ComplianceMonitoring a rdfs:Class,
        owl:Class,
        dpv-owl:OrganisationalMeasure ;
    dct:contributor "Harshvardhan J. Pandit" ;
    dct:created "2022-08-17"^^xsd:date ;
    dct:source [ a schema:WebPage ;
            schema:name "ENISA 5G Cybersecurity Standards" ;
            schema:url "https://www.enisa.europa.eu/publications/5g-cybersecurity-standards" ] ;
    rdfs:isDefinedBy dpv-owl: ;
    rdfs:subClassOf dpv-owl:GovernanceProcedures ;
    sw:term_status "accepted"@en ;
    skos:definition "Monitoring of compliance (e.g. internal policy, regulations)"@en ;
    skos:prefLabel "Compliance Monitoring"@en .

dpv-owl:ComplianceStatus a rdfs:Class,
        owl:Class ;
    dct:contributor "Harshvardhan J. Pandit" ;
    dct:created "2022-05-18"^^xsd:date ;
    vann:example dex-owl:E0055 ;
    rdfs:isDefinedBy dpv-owl: ;
    rdfs:subClassOf dpv-owl:Status ;
    sw:term_status "accepted"@en ;
    skos:definition "Status associated with Compliance with some norms, objectives, or requirements"@en ;
    skos:prefLabel "Compliance Status"@en .

dpv-owl:ComplianceUnknown a rdfs:Class,
        owl:Class,
        dpv-owl:ComplianceStatus ;
    dct:contributor "Harshvardhan J. Pandit" ;
    dct:created "2022-09-07"^^xsd:date ;
    rdfs:isDefinedBy dpv-owl: ;
    rdfs:subClassOf dpv-owl:ComplianceStatus ;
    sw:term_status "accepted"@en ;
    skos:definition "State where the status of compliance is unknown"@en ;
    skos:prefLabel "Compliance Unknown"@en .

dpv-owl:ComplianceViolation a rdfs:Class,
        owl:Class,
        dpv-owl:ComplianceStatus ;
    dct:contributor "Harshvardhan J. Pandit" ;
    dct:created "2022-05-18"^^xsd:date ;
    dct:modified "2022-09-07"^^xsd:date ;
    rdfs:isDefinedBy dpv-owl: ;
    rdfs:subClassOf dpv-owl:ComplianceStatus ;
    sw:term_status "accepted"@en ;
    skos:definition "State where compliance cannot be achieved due to requirements being violated"@en ;
    skos:prefLabel "Compliance Violation"@en ;
    skos:scopeNote "Changed from \"violation of compliance\" for consistency with other terms"@en .

dpv-owl:Compliant a rdfs:Class,
        owl:Class,
        dpv-owl:ComplianceStatus ;
    dct:contributor "Harshvardhan J. Pandit" ;
    dct:created "2022-05-18"^^xsd:date ;
    rdfs:isDefinedBy dpv-owl: ;
    rdfs:subClassOf dpv-owl:ComplianceStatus ;
    sw:term_status "accepted"@en ;
    skos:definition "State of being fully compliant"@en ;
    skos:prefLabel "Compliant"@en .

dpv-owl:ConditionalAutomation a rdfs:Class,
        owl:Class,
        dpv-owl:AutomationLevel ;
    dct:contributor "Harshvardhan J. Pandit, Delaram Golpayegani" ;
    dct:created "2023-12-10"^^xsd:date ;
    dct:modified "2024-04-20"^^xsd:date ;
    dct:source [ a schema:WebPage ;
            schema:name "ISO/IEC 22989:2022 Artificial intelligence concepts and terminology" ;
            schema:url "https://www.iso.org/standard/74296.html" ] ;
    rdfs:isDefinedBy dpv-owl: ;
    rdfs:subClassOf dpv-owl:AutomationLevel ;
    sw:term_status "accepted"@en ;
    skos:definition "Level of automation corresponding to Level 3 in ISO/IEC 22989:2022 where the automation is sufficient to perform most tasks of the system with the human present to take over where necessary"@en ;
    skos:prefLabel "Conditional Automation"@en ;
    skos:scopeNote "Human Involvement is implied here, e.g. for intervention, input, decisions"@en .

dpv-owl:ConfidentialData a rdfs:Class,
        owl:Class ;
    dct:created "2024-02-14"^^xsd:date ;
    dct:source "DGA 5.10"@en ;
    rdfs:isDefinedBy dpv-owl: ;
    rdfs:subClassOf dpv-owl:Data ;
    sw:term_status "accepted"@en ;
    skos:definition "Data deemed confidential"@en ;
    skos:prefLabel "Confidential Data"@en .

dpv-owl:ConfidentialityAgreement a rdfs:Class,
        owl:Class,
        dpv-owl:LegalMeasure ;
    dct:created "2022-02-09"^^xsd:date ;
    dct:source "DGA 3.1.a"@en ;
    rdfs:isDefinedBy dpv-owl: ;
    rdfs:subClassOf dpv-owl:LegalAgreement ;
    sw:term_status "accepted"@en ;
    skos:definition "Agreements that enforce confidentiality for e.g. to protect business, professional, or company secrets"@en ;
    skos:prefLabel "Confidentiality Agreement"@en .

dpv-owl:ConformanceAssessment a rdfs:Class,
        owl:Class,
        dpv-owl:OrganisationalMeasure ;
    dct:contributor "Harshvardhan J. Pandit, Georg P. Krog" ;
    dct:created "2024-04-14"^^xsd:date ;
    rdfs:isDefinedBy dpv-owl: ;
    rdfs:subClassOf dpv-owl:Assessment ;
    sw:term_status "accepted"@en ;
    skos:definition "Assessment regarding conformance with standards or norms or guidelines or similar instruments"@en ;
    skos:prefLabel "Conformance Assessment"@en .

dpv-owl:ConformanceStatus a rdfs:Class,
        owl:Class ;
    dct:contributor "Harshvardhan J. Pandit" ;
    dct:created "2022-10-22"^^xsd:date ;
    rdfs:isDefinedBy dpv-owl: ;
    rdfs:subClassOf dpv-owl:Status ;
    sw:term_status "accepted"@en ;
    skos:definition "Status associated with conformance to a standard, guideline, code, or recommendation"@en ;
    skos:prefLabel "Conformance Status"@en .

dpv-owl:Conformant a rdfs:Class,
        owl:Class,
        dpv-owl:ConformanceStatus ;
    dct:contributor "Harshvardhan J. Pandit" ;
    dct:created "2022-10-22"^^xsd:date ;
    rdfs:isDefinedBy dpv-owl: ;
    rdfs:subClassOf dpv-owl:ConformanceStatus ;
    sw:term_status "accepted"@en ;
    skos:definition "State of being conformant"@en ;
    skos:prefLabel "Conformant"@en .

dpv-owl:Consent a rdfs:Class,
        owl:Class,
        dpv-owl:LegalBasis ;
    dct:contributor "Harshvardhan J. Pandit" ;
    dct:created "2021-04-07"^^xsd:date ;
    vann:example dex-owl:E0015,
        dex-owl:E0018 ;
    rdfs:isDefinedBy dpv-owl: ;
    rdfs:subClassOf dpv-owl:LegalBasis ;
    sw:term_status "accepted"@en ;
    skos:definition "Consent of the Data Subject for specified process or activity"@en ;
    skos:prefLabel "Consent"@en .

dpv-owl:ConsentControl a rdfs:Class,
        owl:Class ;
    dct:created "2024-05-11"^^xsd:date ;
    rdfs:isDefinedBy dpv-owl: ;
    rdfs:subClassOf dpv-owl:EntityInvolvement ;
    sw:term_status "accepted"@en ;
    skos:definition "The control or activity associated with obtaining, providing, withdrawing, or reaffirming consent"@en ;
    skos:prefLabel "Consent Control"@en .

dpv-owl:ConsentExpired a rdfs:Class,
        owl:Class,
        dpv-owl:ConsentStatus ;
    dct:contributor "Georg P. Krog, Harshvardhan J. Pandit, Paul Ryan, Julian Flake" ;
    dct:created "2022-06-22"^^xsd:date ;
    dct:source [ a schema:WebPage ;
            schema:name "GConsent" ;
            schema:url "https://w3id.org/GConsent" ] ;
    rdfs:isDefinedBy dpv-owl: ;
    rdfs:subClassOf dpv-owl:ConsentStatusInvalidForProcessing ;
    sw:term_status "accepted"@en ;
    skos:definition "The state where the temporal or contextual validity of consent has 'expired'"@en ;
    skos:prefLabel "Consent Expired"@en ;
    skos:scopeNote "An example of this state is when the obtained consent has been assigned a duration - which has lapsed or 'expired', making it invalid to be used further for processing data"@en .

dpv-owl:ConsentGiven a rdfs:Class,
        owl:Class,
        dpv-owl:ConsentStatus ;
    dct:contributor "Georg P. Krog, Harshvardhan J. Pandit, Paul Ryan, Julian Flake" ;
    dct:created "2022-06-22"^^xsd:date ;
    dct:source [ a schema:WebPage ;
            schema:name "GConsent" ;
            schema:url "https://w3id.org/GConsent" ] ;
    rdfs:isDefinedBy dpv-owl: ;
    rdfs:subClassOf dpv-owl:ConsentStatusValidForProcessing ;
    sw:term_status "accepted"@en ;
    skos:definition "The state where consent has been given"@en ;
    skos:prefLabel "Consent Given"@en ;
    skos:scopeNote "An example of this state is when the individual clicks on a button, ticks a checkbox, verbally agrees - or any other form that communicates their decision agreeing to the processing of data"@en .

dpv-owl:ConsentInvalidated a rdfs:Class,
        owl:Class,
        dpv-owl:ConsentStatus ;
    dct:contributor "Georg P. Krog, Harshvardhan J. Pandit, Paul Ryan, Julian Flake" ;
    dct:created "2022-06-22"^^xsd:date ;
    dct:source [ a schema:WebPage ;
            schema:name "GConsent" ;
            schema:url "https://w3id.org/GConsent" ] ;
    rdfs:isDefinedBy dpv-owl: ;
    rdfs:subClassOf dpv-owl:ConsentStatusInvalidForProcessing ;
    sw:term_status "accepted"@en ;
    skos:definition "The state where consent has been deemed to be invalid"@en ;
    skos:prefLabel "Consent Invalidated"@en ;
    skos:scopeNote "An example of this state is where an investigating authority or a court finds the collected consent did not meet requirements, and 'invalidates' both prior and future uses of it to carry out processing"@en .

dpv-owl:ConsentManagement a rdfs:Class,
        owl:Class,
        dpv-owl:OrganisationalMeasure ;
    dct:contributor "Beatriz Esteves, Harshvardhan J. Pandit, Georg P. Krog" ;
    dct:created "2024-04-14"^^xsd:date ;
    dct:source "DGA 12.n"@en ;
    rdfs:isDefinedBy dpv-owl: ;
    rdfs:subClassOf dpv-owl:PermissionManagement ;
    sw:term_status "accepted"@en ;
    skos:definition "Methods to obtain, provide, modify, and withdraw consent along with maintaining a record of consent, retrieving records, and processing changes in consent states"@en ;
    skos:prefLabel "Consent Management"@en .

dpv-owl:ConsentNotice a rdfs:Class,
        owl:Class,
        dpv-owl:OrganisationalMeasure ;
    dct:contributor "Georg P. Krog, Harshvardhan J. Pandit, Paul Ryan, Julian Flake" ;
    dct:created "2022-06-21"^^xsd:date ;
    rdfs:isDefinedBy dpv-owl: ;
    rdfs:subClassOf dpv-owl:PrivacyNotice ;
    sw:term_status "accepted"@en ;
    skos:definition "A Notice for information provision associated with Consent"@en ;
    skos:prefLabel "Consent Notice"@en .

dpv-owl:ConsentRecord a rdfs:Class,
        owl:Class,
        dpv-owl:OrganisationalMeasure ;
    dct:contributor "Georg P. Krog, Harshvardhan J. Pandit, Paul Ryan, Julian Flake" ;
    dct:created "2022-06-22"^^xsd:date ;
    vann:example dex-owl:E0016,
        dex-owl:E0023 ;
    rdfs:isDefinedBy dpv-owl: ;
    rdfs:subClassOf dpv-owl:DataProcessingRecord ;
    sw:term_status "accepted"@en ;
    skos:definition "A Record of Consent or Consent related activities"@en ;
    skos:prefLabel "Consent Record"@en .

dpv-owl:ConsentRefused a rdfs:Class,
        owl:Class,
        dpv-owl:ConsentStatus ;
    dct:contributor "Georg P. Krog, Harshvardhan J. Pandit, Paul Ryan, Julian Flake" ;
    dct:created "2022-06-22"^^xsd:date ;
    dct:source [ a schema:WebPage ;
            schema:name "GConsent" ;
            schema:url "https://w3id.org/GConsent" ] ;
    rdfs:isDefinedBy dpv-owl: ;
    rdfs:subClassOf dpv-owl:ConsentStatusInvalidForProcessing ;
    sw:term_status "accepted"@en ;
    skos:definition "The state where consent has been refused"@en ;
    skos:prefLabel "Consent Refused"@en ;
    skos:scopeNote "An example of this state is when the individual clicks on a 'disagree' or 'reject' or 'refuse' button, or leaves a checkbox unticked"@en .

dpv-owl:ConsentRequestDeferred a rdfs:Class,
        owl:Class,
        dpv-owl:ConsentStatus ;
    dct:contributor "Georg P. Krog, Harshvardhan J. Pandit, Paul Ryan, Julian Flake" ;
    dct:created "2022-06-22"^^xsd:date ;
    dct:source [ a schema:WebPage ;
            schema:name "GConsent" ;
            schema:url "https://w3id.org/GConsent" ] ;
    rdfs:isDefinedBy dpv-owl: ;
    rdfs:subClassOf dpv-owl:ConsentStatusInvalidForProcessing ;
    sw:term_status "accepted"@en ;
    skos:definition "State where a request for consent has been deferred without a decision"@en ;
    skos:prefLabel "Consent Request Deferred"@en ;
    skos:scopeNote "An example of this state is when the individual closes or dismisses a notice without making a decision. This state is intended for making the distinction between a notice being provided (as a consent request) and the individual interacting with the notice without making a decision - where the 'ignoring of a notice' is taken as consent being neither given nor refused"@en .

dpv-owl:ConsentRequested a rdfs:Class,
        owl:Class,
        dpv-owl:ConsentStatus ;
    dct:contributor "Georg P. Krog, Harshvardhan J. Pandit, Paul Ryan, Julian Flake" ;
    dct:created "2022-06-22"^^xsd:date ;
    dct:source [ a schema:WebPage ;
            schema:name "GConsent" ;
            schema:url "https://w3id.org/GConsent" ] ;
    rdfs:isDefinedBy dpv-owl: ;
    rdfs:subClassOf dpv-owl:ConsentStatusInvalidForProcessing ;
    sw:term_status "accepted"@en ;
    skos:definition "State where a request for consent has been made and is awaiting a decision"@en ;
    skos:prefLabel "Consent Requested"@en ;
    skos:scopeNote "An example of this state is when a notice has been presented to the individual but they have not made a decision"@en .

dpv-owl:ConsentRevoked a rdfs:Class,
        owl:Class,
        dpv-owl:ConsentStatus ;
    dct:contributor "Georg P. Krog, Harshvardhan J. Pandit, Paul Ryan, Julian Flake" ;
    dct:created "2022-06-22"^^xsd:date ;
    dct:source [ a schema:WebPage ;
            schema:name "GConsent" ;
            schema:url "https://w3id.org/GConsent" ] ;
    rdfs:isDefinedBy dpv-owl: ;
    rdfs:subClassOf dpv-owl:ConsentStatusInvalidForProcessing ;
    sw:term_status "accepted"@en ;
    skos:definition "The state where the consent is revoked by an entity other than the data subject and which prevents it from being further used as a valid state"@en ;
    skos:prefLabel "Consent Revoked"@en ;
    skos:scopeNote "An example of this state is when a Data Controller stops utilising previously obtaining consent, such as when that service no longer exists"@en .

dpv-owl:ConsentStatus a rdfs:Class,
        owl:Class ;
    dct:contributor "Georg P. Krog, Harshvardhan J. Pandit, Paul Ryan, Julian Flake" ;
    dct:created "2022-06-22"^^xsd:date ;
    dct:source [ a schema:WebPage ;
            schema:name "GConsent" ;
            schema:url "https://w3id.org/GConsent" ] ;
    rdfs:isDefinedBy dpv-owl: ;
    rdfs:subClassOf dpv-owl:Status ;
    sw:term_status "accepted"@en ;
    skos:definition "The state or status of 'consent' that provides information reflecting its operational status and validity for processing data"@en ;
    skos:prefLabel "Consent Status"@en ;
    skos:scopeNote "States are useful as information artefacts to implement them in controlling processing, and to reflect the process and flow of obtaining and maintaining consent. For example, a database table that stores consent states for specific processing and can be queried to obtain them in an efficient manner. States are also useful in investigations to determine the use and validity of consenting practices"@en .

dpv-owl:ConsentStatusInvalidForProcessing a rdfs:Class,
        owl:Class,
        dpv-owl:ConsentStatus ;
    dct:contributor "Georg P. Krog, Harshvardhan J. Pandit, Paul Ryan, Julian Flake" ;
    dct:created "2022-06-22"^^xsd:date ;
    dct:source [ a schema:WebPage ;
            schema:name "GConsent" ;
            schema:url "https://w3id.org/GConsent" ] ;
    rdfs:isDefinedBy dpv-owl: ;
    rdfs:subClassOf dpv-owl:ConsentStatus ;
    sw:term_status "accepted"@en ;
    skos:definition "States of consent that cannot be used as valid justifications for processing data"@en ;
    skos:prefLabel "Consent Status Invalid for Processing"@en ;
    skos:scopeNote "This identifies the stages associated with consent that should not be used to process data"@en .

dpv-owl:ConsentStatusValidForProcessing a rdfs:Class,
        owl:Class,
        dpv-owl:ConsentStatus ;
    dct:contributor "Georg P. Krog, Harshvardhan J. Pandit, Paul Ryan, Julian Flake" ;
    dct:created "2022-06-22"^^xsd:date ;
    dct:source [ a schema:WebPage ;
            schema:name "GConsent" ;
            schema:url "https://w3id.org/GConsent" ] ;
    rdfs:isDefinedBy dpv-owl: ;
    rdfs:subClassOf dpv-owl:ConsentStatus ;
    sw:term_status "accepted"@en ;
    skos:definition "States of consent that can be used as valid justifications for processing data"@en ;
    skos:prefLabel "Consent Status Valid for Processing"@en ;
    skos:scopeNote "Practically, given consent is the only valid state for processing"@en .

dpv-owl:ConsentUnknown a rdfs:Class,
        owl:Class,
        dpv-owl:ConsentStatus ;
    dct:contributor "Georg P. Krog, Harshvardhan J. Pandit, Paul Ryan, Julian Flake" ;
    dct:created "2022-06-22"^^xsd:date ;
    dct:source [ a schema:WebPage ;
            schema:name "GConsent" ;
            schema:url "https://w3id.org/GConsent" ] ;
    rdfs:isDefinedBy dpv-owl: ;
    rdfs:subClassOf dpv-owl:ConsentStatusInvalidForProcessing ;
    sw:term_status "accepted"@en ;
    skos:definition "State where information about consent is not available or is unknown"@en ;
    skos:prefLabel "Consent Unknown"@en ;
    skos:scopeNote "Consent states can be unknown, for example, when information is not available, or cannot be trusted, or is known to be inaccurate"@en .

dpv-owl:ConsentWithdrawn a rdfs:Class,
        owl:Class,
        dpv-owl:ConsentStatus ;
    dct:contributor "Georg P. Krog, Harshvardhan J. Pandit, Paul Ryan, Julian Flake" ;
    dct:created "2022-06-22"^^xsd:date ;
    dct:source [ a schema:WebPage ;
            schema:name "GConsent" ;
            schema:url "https://w3id.org/GConsent" ] ;
    rdfs:isDefinedBy dpv-owl: ;
    rdfs:subClassOf dpv-owl:ConsentStatusInvalidForProcessing ;
    sw:term_status "accepted"@en ;
    skos:definition "The state where the consent is withdrawn or revoked specifically by the data subject and which prevents it from being further used as a valid state"@en ;
    skos:prefLabel "Consent Withdrawn"@en ;
    skos:scopeNote "This state can be considered a form of 'revocation' of consent, where the revocation can only be performed by the data subject. Therefore we suggest using ConsentRevoked when it is a non-data-subject entity, and ConsentWithdrawn when it is the data subject"@en .

dpv-owl:Consequence a rdfs:Class,
        owl:Class ;
    dct:contributor "Harshvardhan J. Pandit" ;
    dct:created "2022-01-26"^^xsd:date ;
    vann:example dex-owl:E0027,
        dex-owl:E0068,
        dex-owl:E0071 ;
    rdfs:isDefinedBy dpv-owl: ;
    sw:term_status "accepted"@en ;
    skos:definition "The consequence(s) possible or arising from specified context"@en ;
    skos:prefLabel "Consequence"@en .

dpv-owl:ConsequenceAsSideEffect a rdfs:Class,
        owl:Class ;
    dct:contributor "Harshvardhan J. Pandit" ;
    dct:created "2022-03-30"^^xsd:date ;
    rdfs:isDefinedBy dpv-owl: ;
    rdfs:subClassOf dpv-owl:Consequence ;
    sw:term_status "accepted"@en ;
    skos:definition "The consequence(s) possible or arising as a side-effect of specified context"@en ;
    skos:prefLabel "Consequence as Side-Effect"@en .

dpv-owl:ConsequenceOfFailure a rdfs:Class,
        owl:Class ;
    dct:contributor "Harshvardhan J. Pandit, Georg P. Krog" ;
    dct:created "2022-03-23"^^xsd:date ;
    rdfs:isDefinedBy dpv-owl: ;
    rdfs:subClassOf dpv-owl:Consequence ;
    sw:term_status "accepted"@en ;
    skos:definition "The consequence(s) possible or arising from failure of specified context"@en ;
    skos:prefLabel "Consequence of Failure"@en .

dpv-owl:ConsequenceOfSuccess a rdfs:Class,
        owl:Class ;
    dct:contributor "Harshvardhan J. Pandit, Georg P. Krog" ;
    dct:created "2022-03-23"^^xsd:date ;
    rdfs:isDefinedBy dpv-owl: ;
    rdfs:subClassOf dpv-owl:Consequence ;
    sw:term_status "accepted"@en ;
    skos:definition "The consequence(s) possible or arising from success of specified context"@en ;
    skos:prefLabel "Consequence of Success"@en .

dpv-owl:Consult a rdfs:Class,
        owl:Class,
        dpv-owl:Processing ;
    dct:created "2019-05-07"^^xsd:date ;
    dct:source [ a schema:WebPage ;
            schema:name "SPECIAL Project" ;
            schema:url "https://specialprivacy.ercim.eu/vocabs/processing" ],
        [ a schema:WebPage ;
            schema:name "GDPR Art.4-2" ;
            schema:url "https://eur-lex.europa.eu/eli/reg/2016/679/art_4/par_2/oj" ] ;
    rdfs:isDefinedBy dpv-owl: ;
    rdfs:subClassOf dpv-owl:Use ;
    sw:term_status "accepted"@en ;
    skos:definition "to consult or query data"@en ;
    skos:prefLabel "Consult"@en ;
    skos:related svpr:Query .

dpv-owl:Consultation a rdfs:Class,
        owl:Class,
        dpv-owl:OrganisationalMeasure ;
    dct:contributor "Georg P. Krog, Harshvardhan J. Pandit, Paul Ryan" ;
    dct:created "2020-11-04"^^xsd:date ;
    rdfs:isDefinedBy dpv-owl: ;
    rdfs:subClassOf dpv-owl:OrganisationalMeasure ;
    sw:term_status "accepted"@en ;
    skos:definition "Consultation is a process of receiving feedback, advice, or opinion from an external agency"@en ;
    skos:prefLabel "Consultation"@en .

dpv-owl:ConsultationWithAuthority a rdfs:Class,
        owl:Class,
        dpv-owl:OrganisationalMeasure ;
    dct:contributor "Georg P. Krog, Harshvardhan J. Pandit, Paul Ryan" ;
    dct:created "2020-11-04"^^xsd:date ;
    rdfs:isDefinedBy dpv-owl: ;
    rdfs:subClassOf dpv-owl:Consultation ;
    sw:term_status "accepted"@en ;
    skos:definition "Consultation with an authority or authoritative entity"@en ;
    skos:prefLabel "Consultation with Authority"@en .

dpv-owl:ConsultationWithDPO a rdfs:Class,
        owl:Class,
        dpv-owl:OrganisationalMeasure ;
    dct:contributor "Harshvardhan J. Pandit, Georg P. Krog" ;
    dct:created "2022-06-15"^^xsd:date ;
    rdfs:isDefinedBy dpv-owl: ;
    rdfs:subClassOf dpv-owl:Consultation ;
    sw:term_status "accepted"@en ;
    skos:definition "Consultation with Data Protection Officer(s)"@en ;
    skos:prefLabel "Consultation with DPO"@en .

dpv-owl:ConsultationWithDataSubject a rdfs:Class,
        owl:Class,
        dpv-owl:OrganisationalMeasure ;
    dct:contributor "Harshvardhan J. Pandit, Georg P. Krog" ;
    dct:created "2022-06-15"^^xsd:date ;
    rdfs:isDefinedBy dpv-owl: ;
    rdfs:subClassOf dpv-owl:Consultation ;
    sw:term_status "accepted"@en ;
    skos:definition "Consultation with data subject(s) or their representative(s)"@en ;
    skos:prefLabel "Consultation with Data Subject"@en .

dpv-owl:ConsultationWithDataSubjectRepresentative a rdfs:Class,
        owl:Class,
        dpv-owl:OrganisationalMeasure ;
    dct:contributor "Harshvardhan J. Pandit, Georg P. Krog" ;
    dct:created "2022-10-22"^^xsd:date ;
    rdfs:isDefinedBy dpv-owl: ;
    rdfs:subClassOf dpv-owl:ConsultationWithDataSubject ;
    sw:term_status "accepted"@en ;
    skos:definition "Consultation with representative of data subject(s)"@en ;
    skos:prefLabel "Consultation with Data Subject Representative"@en .

dpv-owl:Consumer a rdfs:Class,
        owl:Class,
        dpv-owl:DataSubject ;
    dct:contributor "Harshvardhan J. Pandit, Georg P. Krog, Julian Flake, Paul Ryan, Beatriz Esteves" ;
    dct:created "2022-04-06"^^xsd:date ;
    rdfs:isDefinedBy dpv-owl: ;
    rdfs:subClassOf dpv-owl:DataSubject ;
    sw:term_status "accepted"@en ;
    skos:definition "Data subjects that consume goods or services for direct use"@en ;
    skos:prefLabel "Consumer"@en .

dpv-owl:Context a rdfs:Class,
        owl:Class ;
    dct:contributor "Harshvardhan J. Pandit, Javier Fernández, Axel Polleres, Elmar Kiesling, Fajar Ekaputra, Simon Steyskal" ;
    dct:created "2019-04-05"^^xsd:date ;
    dct:modified "2022-06-15"^^xsd:date ;
    rdfs:isDefinedBy dpv-owl: ;
    sw:term_status "accepted"@en ;
    skos:definition "Contextually relevant information"@en ;
    skos:prefLabel "Context"@en ;
    skos:scopeNote "Context is a catch-all concept for information of relevance not possible to represent through other core concepts. DPV offers specific contextual concepts such as Necessity, Frequency, and Duration. More can be created by extending Context within use-cases."@en .

dpv-owl:ContextuallyAnonymisedData a rdfs:Class,
        owl:Class ;
    dct:contributor "Harshvardhan J. Pandit" ;
    dct:created "2024-06-11"^^xsd:date ;
    rdfs:isDefinedBy dpv-owl: ;
    rdfs:subClassOf dpv-owl:PseudonymisedData ;
    sw:term_status "accepted"@en ;
    skos:definition "Data that can be considered as being fully anonymised within the context but in actuality is not fully anonymised and is still personal data as it can be de-anonymised outside that context"@en ;
    skos:prefLabel "Contextually Anonymised Data"@en ;
    skos:scopeNote "To distinguish between partially anonymised data that can be effectively treated as anonymised data (e.g. in processing) within a context (e.g. an organisation), the concept ContextuallyAnonymisedData should be used instead of AnonymisedData. Transfer of this data outside of the context should consider that it is not fully anonymised and that it is still personal data"@en .

dpv-owl:ContinuousFrequency a rdfs:Class,
        owl:Class,
        dpv-owl:Frequency ;
    dct:contributor "Harshvardhan J. Pandit" ;
    dct:created "2022-06-15"^^xsd:date ;
    dct:modified "2020-10-05"^^xsd:date ;
    rdfs:isDefinedBy dpv-owl: ;
    rdfs:subClassOf dpv-owl:Frequency ;
    sw:term_status "accepted"@en ;
    skos:definition "Frequency where occurrences are continuous"@en ;
    skos:prefLabel "Continuous Frequency"@en .

dpv-owl:Contract a rdfs:Class,
        owl:Class,
        dpv-owl:LegalBasis ;
    dct:contributor "Harshvardhan J. Pandit" ;
    dct:created "2021-04-07"^^xsd:date ;
    rdfs:isDefinedBy dpv-owl: ;
    rdfs:subClassOf dpv-owl:LegalAgreement ;
    sw:term_status "accepted"@en ;
    skos:definition "Creation, completion, fulfilment, or performance of a contract involving specified processing of data or technologies"@en ;
    skos:prefLabel "Contract"@en .

dpv-owl:ContractPerformance a rdfs:Class,
        owl:Class,
        dpv-owl:LegalBasis ;
    dct:contributor "Georg P. Krog, Harshvardhan J. Pandit, Paul Ryan" ;
    dct:created "2021-04-07"^^xsd:date ;
    rdfs:isDefinedBy dpv-owl: ;
    rdfs:subClassOf dpv-owl:Contract ;
    sw:term_status "accepted"@en ;
    skos:definition "Fulfilment or performance of a contract involving specified processing of data or technologies"@en ;
    skos:prefLabel "Contract Performance"@en .

dpv-owl:ContractualTerms a rdfs:Class,
        owl:Class,
        dpv-owl:LegalMeasure ;
    dct:contributor "Axel Polleres, Rob Brennan, Harshvardhan J. Pandit, Mark Lizar" ;
    dct:created "2019-04-05"^^xsd:date ;
    rdfs:isDefinedBy dpv-owl: ;
    rdfs:subClassOf dpv-owl:LegalAgreement ;
    sw:term_status "accepted"@en ;
    skos:definition "Contractual terms governing data handling within or with an entity"@en ;
    skos:prefLabel "Contractual Terms"@en .

dpv-owl:ControllerInformed a rdfs:Class,
        owl:Class,
        dpv-owl:EntityInformedStatus ;
    dct:contributor "Harshvardhan J. Pandit, Delaram Golpayegani, Georg P. Krog, Paul Ryan" ;
    dct:created "2024-05-10"^^xsd:date ;
    rdfs:isDefinedBy dpv-owl: ;
    rdfs:subClassOf dpv-owl:EntityInformed ;
    sw:term_status "accepted"@en ;
    skos:definition "Status indicating Controller has been informed about the specified context"@en ;
    skos:prefLabel "Controller Informed"@en .

dpv-owl:ControllerProcessorAgreement a rdfs:Class,
        owl:Class,
        dpv-owl:LegalMeasure ;
    dct:contributor "Georg P. Krog, Harshvardhan J. Pandit, Beatriz Esteves, Paul Ryan, Julian Flake" ;
    dct:created "2022-01-26"^^xsd:date ;
    vann:example dex-owl:E0024 ;
    rdfs:isDefinedBy dpv-owl: ;
    rdfs:subClassOf dpv-owl:DataProcessingAgreement ;
    sw:term_status "accepted"@en ;
    skos:definition "An agreement outlining conditions, criteria, obligations, responsibilities, and specifics for carrying out processing of data between a Data Controller and a Data Processor"@en ;
    skos:prefLabel "Controller-Processor Agreement"@en .

dpv-owl:ControllerUninformed a rdfs:Class,
        owl:Class,
        dpv-owl:EntityInformedStatus ;
    dct:contributor "Harshvardhan J. Pandit, Delaram Golpayegani, Georg P. Krog, Paul Ryan" ;
    dct:created "2024-05-10"^^xsd:date ;
    rdfs:isDefinedBy dpv-owl: ;
    rdfs:subClassOf dpv-owl:EntityUninformed ;
    sw:term_status "accepted"@en ;
    skos:definition "Status indicating Controller is uninformed i.e. has not been informed about the specified context"@en ;
    skos:prefLabel "Controller Uninformed"@en .

dpv-owl:Copy a rdfs:Class,
        owl:Class,
        dpv-owl:Processing ;
    dct:created "2019-05-07"^^xsd:date ;
    dct:source [ a schema:WebPage ;
            schema:name "SPECIAL Project" ;
            schema:url "https://specialprivacy.ercim.eu/vocabs/processing" ] ;
    rdfs:isDefinedBy dpv-owl: ;
    rdfs:subClassOf dpv-owl:Processing ;
    sw:term_status "accepted"@en ;
    skos:definition "to produce an exact reproduction of the data"@en ;
    skos:prefLabel "Copy"@en ;
    skos:related svpr:Copy .

dpv-owl:CorrectingProcess a rdfs:Class,
        owl:Class,
        dpv-owl:EntityPermissiveInvolvement ;
    dct:contributor "Harshvardhan J. Pandit, Delaram Golpayegani, Steve Hickman" ;
    dct:created "2024-05-11"^^xsd:date ;
    rdfs:isDefinedBy dpv-owl: ;
    rdfs:subClassOf dpv-owl:EntityPermissiveInvolvement ;
    sw:term_status "accepted"@en ;
    skos:definition "Involvement where entity can correct the process of specified context"@en ;
    skos:prefLabel "Correcting Process"@en ;
    skos:scopeNote "Correction of process refers to the ability to change how the process takes place"@en .

dpv-owl:CorrectingProcessInput a rdfs:Class,
        owl:Class,
        dpv-owl:EntityPermissiveInvolvement ;
    dct:contributor "Harshvardhan J. Pandit, Delaram Golpayegani, Steve Hickman" ;
    dct:created "2024-05-11"^^xsd:date ;
    rdfs:isDefinedBy dpv-owl: ;
    rdfs:subClassOf dpv-owl:EntityPermissiveInvolvement ;
    sw:term_status "accepted"@en ;
    skos:definition "Involvement where entity can correct input of specified context"@en ;
    skos:prefLabel "Correcting Process Input"@en .

dpv-owl:CorrectingProcessOutput a rdfs:Class,
        owl:Class,
        dpv-owl:EntityPermissiveInvolvement ;
    dct:contributor "Harshvardhan J. Pandit, Delaram Golpayegani, Steve Hickman" ;
    dct:created "2024-05-11"^^xsd:date ;
    rdfs:isDefinedBy dpv-owl: ;
    rdfs:subClassOf dpv-owl:EntityPermissiveInvolvement ;
    sw:term_status "accepted"@en ;
    skos:definition "Involvement where entity can correct the output of specified context"@en ;
    skos:prefLabel "Correcting Process Output"@en ;
    skos:scopeNote "Correction of outputs allows modification of the output - implying continuation of the process. This is distinct from reversing of outputs which revert the output back to its previous value and possibly imply not continuing with the process"@en .

dpv-owl:CounterMoneyLaundering a rdfs:Class,
        owl:Class,
        dpv-owl:Purpose ;
    dct:contributor "Harshvardhan J. Pandit" ;
    dct:created "2022-04-20"^^xsd:date ;
    rdfs:isDefinedBy dpv-owl: ;
    rdfs:subClassOf dpv-owl:FraudPreventionAndDetection ;
    sw:term_status "accepted"@en ;
    skos:definition "Purposes associated with detection, prevention, and mitigation of mitigate money laundering"@en ;
    skos:prefLabel "Counter Money Laundering"@en .

dpv-owl:Counterterrorism a rdfs:Class,
        owl:Class,
        dpv-owl:Purpose ;
    dct:contributor "Harshvardhan J. Pandit" ;
    dct:created "2022-04-20"^^xsd:date ;
    dct:modified "2024-04-14"^^xsd:date ;
    rdfs:isDefinedBy dpv-owl: ;
    rdfs:subClassOf dpv-owl:PublicBenefit ;
    sw:term_status "accepted"@en ;
    skos:definition "Purposes associated with activities that detect, prevent, mitigate, or otherwise perform activities to combat or eliminate terrorism (also referred to as anti-terrorism)"@en ;
    skos:prefLabel "Counterterrorism"@en .

dpv-owl:Country a rdfs:Class,
        owl:Class ;
    dct:contributor "Harshvardhan J. Pandit, Georg P. Krog" ;
    dct:created "2022-01-19"^^xsd:date ;
    rdfs:isDefinedBy dpv-owl: ;
    rdfs:subClassOf dpv-owl:Location ;
    sw:term_status "accepted"@en ;
    skos:definition "A political entity indicative of a sovereign or non-sovereign territorial state comprising of distinct geographical areas"@en ;
    skos:prefLabel "Country"@en ;
    skos:scopeNote "The definition of country is not intended for political interpretation. DPVCG welcomes alternate definitions based in existing sources with global scope, such as UN or ISO."@en .

dpv-owl:CredentialManagement a rdfs:Class,
        owl:Class,
        dpv-owl:OrganisationalMeasure ;
    dct:contributor "Georg P. Krog" ;
    dct:created "2022-06-15"^^xsd:date ;
    rdfs:isDefinedBy dpv-owl: ;
    rdfs:subClassOf dpv-owl:AuthorisationProcedure ;
    sw:term_status "accepted"@en ;
    skos:definition "Management of credentials and their use in authorisations"@en ;
    skos:prefLabel "Credential Management"@en .

dpv-owl:CreditChecking a rdfs:Class,
        owl:Class,
        dpv-owl:Purpose ;
    dct:contributor "Harshvardhan J. Pandit" ;
    dct:created "2022-04-20"^^xsd:date ;
    rdfs:isDefinedBy dpv-owl: ;
    rdfs:subClassOf dpv-owl:CustomerSolvencyMonitoring ;
    sw:term_status "accepted"@en ;
    skos:definition "Purposes associated with monitoring, performing, or assessing credit worthiness or solvency"@en ;
    skos:prefLabel "Credit Checking"@en .

dpv-owl:CrossBorderTransfer a rdfs:Class,
        owl:Class,
        dpv-owl:Processing ;
    dct:contributor "Harshvardhan J. Pandit" ;
    dct:created "2024-04-14"^^xsd:date ;
    rdfs:isDefinedBy dpv-owl: ;
    rdfs:subClassOf dpv-owl:Transfer ;
    sw:term_status "accepted"@en ;
    skos:definition "to move data from one jurisdiction (border) to another"@en ;
    skos:prefLabel "Cross-Border Transfer"@en .

dpv-owl:CryptographicAuthentication a rdfs:Class,
        owl:Class,
        dpv-owl:TechnicalMeasure ;
    dct:contributor "Harshvardhan J. Pandit" ;
    dct:created "2022-08-17"^^xsd:date ;
    dct:source [ a schema:WebPage ;
            schema:name "ENISA Reference Incident Classification Taxonomy 2018" ;
            schema:url "https://www.enisa.europa.eu/publications/reference-incident-classification-taxonomy/" ] ;
    rdfs:isDefinedBy dpv-owl: ;
    rdfs:subClassOf dpv-owl:AuthenticationProtocols,
        dpv-owl:CryptographicMethods ;
    sw:term_status "accepted"@en ;
    skos:definition "Use of cryptography for authentication"@en ;
    skos:prefLabel "Cryptographic Authentication"@en .

dpv-owl:CryptographicKeyManagement a rdfs:Class,
        owl:Class,
        dpv-owl:TechnicalMeasure ;
    dct:contributor "Harshvardhan J. Pandit" ;
    dct:created "2022-08-17"^^xsd:date ;
    dct:source [ a schema:WebPage ;
            schema:name "ENISA Reference Incident Classification Taxonomy 2018" ;
            schema:url "https://www.enisa.europa.eu/publications/reference-incident-classification-taxonomy/" ] ;
    rdfs:isDefinedBy dpv-owl: ;
    rdfs:subClassOf dpv-owl:CryptographicMethods ;
    sw:term_status "accepted"@en ;
    skos:definition "Management of cryptographic keys, including their generation, storage, assessment, and safekeeping"@en ;
    skos:prefLabel "Cryptographic Key Management"@en .

dpv-owl:CryptographicMethods a rdfs:Class,
        owl:Class,
        dpv-owl:TechnicalMeasure ;
    dct:contributor "Harshvardhan J. Pandit" ;
    dct:created "2022-08-17"^^xsd:date ;
    dct:source [ a schema:WebPage ;
            schema:name "ENISA Reference Incident Classification Taxonomy 2018" ;
            schema:url "https://www.enisa.europa.eu/publications/reference-incident-classification-taxonomy/" ] ;
    rdfs:isDefinedBy dpv-owl: ;
    rdfs:subClassOf dpv-owl:TechnicalMeasure ;
    sw:term_status "accepted"@en ;
    skos:definition "Use of cryptographic methods to perform tasks"@en ;
    skos:prefLabel "Cryptographic Methods"@en .

dpv-owl:Customer a rdfs:Class,
        owl:Class,
        dpv-owl:DataSubject ;
    dct:contributor "Harshvardhan J. Pandit, Georg P. Krog, Julian Flake, Paul Ryan, Beatriz Esteves" ;
    dct:created "2022-04-06"^^xsd:date ;
    rdfs:isDefinedBy dpv-owl: ;
    rdfs:subClassOf dpv-owl:DataSubject ;
    sw:term_status "accepted"@en ;
    skos:definition "Data subjects that purchase goods or services"@en ;
    skos:prefLabel "Customer"@en ;
    skos:scopeNote "note: for B2B relations where customers are organisations, this concept only applies for data subjects"@en .

dpv-owl:CustomerCare a rdfs:Class,
        owl:Class,
        dpv-owl:Purpose ;
    dct:contributor "Harshvardhan J. Pandit, Javier Fernández, Axel Polleres, Elmar Kiesling, Fajar Ekaputra, Simon Steyskal" ;
    dct:created "2019-04-05"^^xsd:date ;
    rdfs:isDefinedBy dpv-owl: ;
    rdfs:subClassOf dpv-owl:CustomerManagement ;
    sw:term_status "accepted"@en ;
    skos:definition "Customer Care refers to purposes associated with purposes for providing assistance, resolving issues, ensuring satisfaction, etc. in relation to services provided"@en ;
    skos:prefLabel "Customer Care"@en ;
    skos:related svpu:Feedback .

dpv-owl:CustomerClaimsManagement a rdfs:Class,
        owl:Class,
        dpv-owl:Purpose ;
    dct:contributor "Georg P. Krog, Harshvardhan J. Pandit, Beatriz Esteves" ;
    dct:created "2021-09-08"^^xsd:date ;
    dct:source [ a schema:WebPage ;
            schema:name "Belgian DPA ROPA Template" ;
            schema:url "https://www.privacycommission.be/nl/model-voor-een-register-van-de-verwerkingsactiviteiten" ] ;
    rdfs:isDefinedBy dpv-owl: ;
    rdfs:subClassOf dpv-owl:CustomerManagement ;
    sw:term_status "accepted"@en ;
    skos:definition "Customer Claims Management refers to purposes associated with managing claims, including repayment of monies owed"@en ;
    skos:prefLabel "Customer Claims Management"@en .

dpv-owl:CustomerManagement a rdfs:Class,
        owl:Class,
        dpv-owl:Purpose ;
    dct:contributor "Georg P. Krog, Harshvardhan J. Pandit, Beatriz Esteves" ;
    dct:created "2021-09-08"^^xsd:date ;
    rdfs:isDefinedBy dpv-owl: ;
    rdfs:subClassOf dpv-owl:Purpose ;
    sw:term_status "accepted"@en ;
    skos:definition "Customer Management refers to purposes associated with managing activities related with past, current, and future customers"@en ;
    skos:prefLabel "Customer Management"@en .

dpv-owl:CustomerOrderManagement a rdfs:Class,
        owl:Class,
        dpv-owl:Purpose ;
    dct:contributor "Georg P. Krog, Harshvardhan J. Pandit, Beatriz Esteves" ;
    dct:created "2021-09-08"^^xsd:date ;
    dct:source [ a schema:WebPage ;
            schema:name "Belgian DPA ROPA Template" ;
            schema:url "https://www.privacycommission.be/nl/model-voor-een-register-van-de-verwerkingsactiviteiten" ] ;
    rdfs:isDefinedBy dpv-owl: ;
    rdfs:subClassOf dpv-owl:CustomerManagement ;
    sw:term_status "accepted"@en ;
    skos:definition "Customer Order Management refers to purposes associated with managing customer orders i.e. processing of an order related to customer's purchase of good or services"@en ;
    skos:prefLabel "Customer Order Management"@en .

dpv-owl:CustomerRelationshipManagement a rdfs:Class,
        owl:Class,
        dpv-owl:Purpose ;
    dct:contributor "Georg P. Krog, Harshvardhan J. Pandit, Beatriz Esteves" ;
    dct:created "2021-09-08"^^xsd:date ;
    rdfs:isDefinedBy dpv-owl: ;
    rdfs:subClassOf dpv-owl:CustomerManagement ;
    sw:term_status "accepted"@en ;
    skos:definition "Customer Relationship Management refers to purposes associated with managing and analysing interactions with past, current, and potential customers"@en ;
    skos:prefLabel "Customer Relationship Management"@en .

dpv-owl:CustomerSolvencyMonitoring a rdfs:Class,
        owl:Class,
        dpv-owl:Purpose ;
    dct:contributor "Georg P. Krog, Harshvardhan J. Pandit, Beatriz Esteves" ;
    dct:created "2021-09-08"^^xsd:date ;
    dct:source [ a schema:WebPage ;
            schema:name "Belgian DPA ROPA Template" ;
            schema:url "https://www.privacycommission.be/nl/model-voor-een-register-van-de-verwerkingsactiviteiten" ] ;
    rdfs:isDefinedBy dpv-owl: ;
    rdfs:subClassOf dpv-owl:CustomerManagement ;
    sw:term_status "accepted"@en ;
    skos:definition "Customer Solvency Monitoring refers to purposes associated with monitor solvency of customers for financial diligence"@en ;
    skos:prefLabel "Customer Solvency Monitoring"@en .

dpv-owl:CybersecurityAssessment a rdfs:Class,
        owl:Class,
        dpv-owl:OrganisationalMeasure ;
    dct:contributor "Harshvardhan J. Pandit" ;
    dct:created "2022-08-17"^^xsd:date ;
    dct:source [ a schema:WebPage ;
            schema:name "ENISA 5G Cybersecurity Standards" ;
            schema:url "https://www.enisa.europa.eu/publications/5g-cybersecurity-standards" ] ;
    rdfs:isDefinedBy dpv-owl: ;
    rdfs:subClassOf dpv-owl:SecurityAssessment ;
    sw:term_status "accepted"@en ;
    skos:definition "Assessment of cybersecurity capabilities in terms of vulnerabilities and effectiveness of controls"@en ;
    skos:prefLabel "Cybersecurity Assessment"@en .

dpv-owl:CybersecurityTraining a rdfs:Class,
        owl:Class,
        dpv-owl:OrganisationalMeasure ;
    dct:contributor "Harshvardhan J. Pandit" ;
    dct:created "2022-08-17"^^xsd:date ;
    dct:source [ a schema:WebPage ;
            schema:name "ENISA Reference Incident Classification Taxonomy 2018" ;
            schema:url "https://www.enisa.europa.eu/publications/reference-incident-classification-taxonomy/" ] ;
    rdfs:isDefinedBy dpv-owl: ;
    rdfs:subClassOf dpv-owl:StaffTraining ;
    sw:term_status "accepted"@en ;
    skos:definition "Training methods related to cybersecurity"@en ;
    skos:prefLabel "Cybersecurity Training"@en .

dpv-owl:DPIA a rdfs:Class,
        owl:Class,
        dpv-owl:OrganisationalMeasure ;
    dct:contributor "Georg P. Krog, Harshvardhan J. Pandit, Paul Ryan" ;
    dct:created "2020-11-04"^^xsd:date ;
    dct:modified "2024-04-14"^^xsd:date ;
    dct:source "GDPR Art. 35"@en ;
    vann:example dex-owl:E0056 ;
    rdfs:isDefinedBy dpv-owl: ;
    rdfs:subClassOf dpv-owl:RightsImpactAssessment ;
    sw:term_status "accepted"@en ;
    skos:definition "Impact assessment determining the potential and actual impact of processing activities on individuals or groups of individuals and taking into account the impacts of activities on their rights and freedoms"@en ;
    skos:prefLabel "Data Protection Impact Assessment (DPIA)"@en ;
    skos:scopeNote "Specific requirements and procedures for DPIA are defined in GDPR Art.35"@en .

dpv-owl:Data a rdfs:Class,
        owl:Class ;
    dct:contributor "Harshvardhan J. Pandit" ;
    dct:created "2022-01-19"^^xsd:date ;
    rdfs:isDefinedBy dpv-owl: ;
    sw:term_status "accepted"@en ;
    skos:definition "A broad concept representing  'data' or 'information'"@en ;
    skos:prefLabel "Data"@en .

dpv-owl:DataAltruism a rdfs:Class,
        owl:Class,
        dpv-owl:Purpose ;
    dct:contributor "Beatriz Esteves, Harshvardhan J. Pandit" ;
    dct:created "2024-02-14"^^xsd:date ;
    dct:source "DGA 2.16"@en ;
    rdfs:isDefinedBy dpv-owl: ;
    rdfs:subClassOf dpv-owl:PublicBenefit ;
    sw:term_status "accepted"@en ;
    skos:definition "Purposes associated with the voluntary sharing of data for the general interest of the public, such as healthcare or combating climate change"@en ;
    skos:prefLabel "Data Altruism"@en ;
    skos:scopeNote "Data Altruism as a purpose should be combined with other purposes to indicate their altruistic interpretation or application. E.g. improving healthcare and data altruism in combination."@en .

dpv-owl:DataBackupProtocols a rdfs:Class,
        owl:Class,
        dpv-owl:TechnicalMeasure ;
    dct:contributor "Georg P. Krog" ;
    dct:created "2022-06-15"^^xsd:date ;
    rdfs:isDefinedBy dpv-owl: ;
    rdfs:subClassOf dpv-owl:TechnicalMeasure ;
    sw:term_status "accepted"@en ;
    skos:definition "Protocols or plans for backing up of data"@en ;
    skos:prefLabel "Data Backup Protocols"@en .

dpv-owl:DataBreachImpactAssessment a rdfs:Class,
        owl:Class,
        dpv-owl:OrganisationalMeasure ;
    dct:contributor "Harshvardhan J. Pandit" ;
    dct:created "2024-04-15"^^xsd:date ;
    rdfs:isDefinedBy dpv-owl: ;
    rdfs:subClassOf dpv-owl:RightsImpactAssessment ;
    sw:term_status "accepted"@en ;
    skos:definition "Impact Assessment concerning the consequences and impacts of a data breach"@en ;
    skos:prefLabel "Data Breach Impact Assessment (DBIA)"@en ;
    skos:scopeNote "Data Breach assessments can require additional non-security related assessments such as GDPR Art.34 Rights Impact Assessment"@en .

dpv-owl:DataBreachNotice a rdfs:Class,
        owl:Class,
        dpv-owl:OrganisationalMeasure ;
    dct:contributor "Georg P. Krog, Paul Ryan, David Hickey, Beatriz Esteves, Harshvardhan J. Pandit" ;
    dct:created "2024-04-14"^^xsd:date ;
    dct:source " DGA 21.5 GDPR 33"@en,
        " GDPR 34"@en,
        "DGA 12.k"@en ;
    rdfs:isDefinedBy dpv-owl: ;
    rdfs:subClassOf dpv-owl:SecurityIncidentNotice ;
    sw:term_status "accepted"@en ;
    skos:definition "A notice providing information about data breach(es) i.e. unauthorised transfer, access, use, or modification of data"@en ;
    skos:prefLabel "Data Breach Notice"@en .

dpv-owl:DataBreachNotification a rdfs:Class,
        owl:Class,
        dpv-owl:OrganisationalMeasure ;
    dct:contributor "Harshvardhan J. Pandit" ;
    dct:created "2024-04-14"^^xsd:date ;
    dct:source " DGA 21.5 GDPR 33"@en,
        " GDPR 34"@en,
        "DGA 12.k"@en ;
    rdfs:isDefinedBy dpv-owl: ;
    rdfs:subClassOf dpv-owl:SecurityIncidentNotification ;
    sw:term_status "accepted"@en ;
    skos:definition "Notification of information about data breach(es) i.e. unauthorised transfer, access, use, or modification of data"@en ;
    skos:prefLabel "Data Breach Notification"@en .

dpv-owl:DataBreachRecord a rdfs:Class,
        owl:Class,
        dpv-owl:OrganisationalMeasure ;
    dct:contributor "Harshvardhan J. Pandit" ;
    dct:created "2024-04-14"^^xsd:date ;
    rdfs:isDefinedBy dpv-owl: ;
    rdfs:subClassOf dpv-owl:RecordsOfActivities ;
    sw:term_status "accepted"@en ;
    skos:definition "Record of a data breach incident"@en ;
    skos:prefLabel "Data Breach Record"@en .

dpv-owl:DataController a rdfs:Class,
        owl:Class ;
    dct:contributor "Axel Polleres, Javier Fernández" ;
    dct:created "2019-04-05"^^xsd:date ;
    dct:modified "2020-11-04"^^xsd:date ;
    dct:source [ a schema:WebPage ;
            schema:name "GDPR Art.4-7g" ;
            schema:url "https://eur-lex.europa.eu/eli/reg/2016/679/art_4/par_7/oj" ] ;
    vann:example dex-owl:E0032,
        dex-owl:E0033 ;
    rdfs:isDefinedBy dpv-owl: ;
    rdfs:subClassOf dpv-owl:LegalEntity ;
    sw:term_status "accepted"@en ;
    skos:definition "The individual or organisation that decides (or controls) the purpose(s) of processing personal data."@en ;
    skos:prefLabel "Data Controller"@en ;
    skos:scopeNote "The terms 'Controller', 'Data Controller', and 'PII Controller' refer to the same concept"@en .

dpv-owl:DataControllerContract a rdfs:Class,
        owl:Class,
        dpv-owl:LegalBasis ;
    dct:created "2023-12-10"^^xsd:date ;
    rdfs:isDefinedBy dpv-owl: ;
    rdfs:subClassOf dpv-owl:Contract ;
    sw:term_status "accepted"@en ;
    skos:definition "Creation, completion, fulfilment, or performance of a contract, with Data Controllers as parties being Joint Data Controllers, and involving specified processing of data or technologies"@en ;
    skos:prefLabel "Data Controller Contract"@en .

dpv-owl:DataControllerDataSource a rdfs:Class,
        owl:Class,
        dpv-owl:DataSource ;
    dct:created "2023-10-12"^^xsd:date ;
    rdfs:isDefinedBy dpv-owl: ;
    rdfs:subClassOf dpv-owl:DataSource ;
    sw:term_status "accepted"@en ;
    skos:definition "Data Sourced from Data Controller(s), e.g. a Controller inferring data or generating data"@en ;
    skos:prefLabel "Data Controller as Data Source"@en .

dpv-owl:DataDeletionPolicy a rdfs:Class,
        owl:Class,
        dpv-owl:OrganisationalMeasure ;
    dct:contributor "Georg P. Krog, Harshvardhan J. Pandit" ;
    dct:created "2024-04-14"^^xsd:date ;
    rdfs:isDefinedBy dpv-owl: ;
    rdfs:subClassOf dpv-owl:DataProcessingPolicy ;
    sw:term_status "accepted"@en ;
    skos:definition "Policy regarding deletion of data"@en ;
    skos:prefLabel "Data Deletion Policy"@en ;
    skos:scopeNote "Deletion and Erasure are distinct activities where deletion refers to logical removal of data with the possibility of retrieval whereas erasure refers to destruction of data such that it cannot be retrieved. See dpv:DataErasurePolicy"@en .

dpv-owl:DataErasurePolicy a rdfs:Class,
        owl:Class,
        dpv-owl:OrganisationalMeasure ;
    dct:contributor "Harshvardhan J. Pandit" ;
    dct:created "2024-04-14"^^xsd:date ;
    rdfs:isDefinedBy dpv-owl: ;
    rdfs:subClassOf dpv-owl:DataProcessingPolicy ;
    sw:term_status "accepted"@en ;
    skos:definition "Policy regarding erasure of data"@en ;
    skos:prefLabel "Data Erasure Policy"@en ;
    skos:scopeNote "Erasure or data destruction or secure removal of data refers to irreversible erasure of data. See dpv:DataDeletion for reversible or logical deletion of data"@en .

dpv-owl:DataExporter a rdfs:Class,
        owl:Class ;
    dct:contributor "David Hickey, Georg P. Krog, Paul Ryan, Harshvardhan J. Pandit" ;
    dct:created "2021-09-08"^^xsd:date ;
    dct:source [ a schema:WebPage ;
            schema:name "EDPB Recommendations 01/2020 on Data Transfers" ;
            schema:url "https://edpb.europa.eu/our-work-tools/our-documents/recommendations/recommendations-012020-measures-supplement-transfer_en" ] ;
    vann:example dex-owl:E0035 ;
    rdfs:isDefinedBy dpv-owl: ;
    rdfs:subClassOf dpv-owl:LegalEntity ;
    sw:term_status "accepted"@en ;
    skos:definition "An entity that 'exports' data where exporting is considered a form of data transfer"@en ;
    skos:prefLabel "Data Exporter"@en ;
    skos:scopeNote "The term 'Data Exporter' is used by the EU-EDPB as the entity that transfer data across borders. While the EDPB refers to the jurisdictional border of EU, the term within DPV can be used to denote any 'export' or transfer or transmission of data and is thus a broader concept than the EDPB's definition."@en .

dpv-owl:DataGovernance a rdfs:Class,
        owl:Class,
        dpv-owl:OrganisationalMeasure ;
    dct:contributor "Harshvardhan J. Pandit" ;
    dct:created "2024-04-14"^^xsd:date ;
    rdfs:isDefinedBy dpv-owl: ;
    rdfs:subClassOf dpv-owl:OrganisationGovernance ;
    sw:term_status "accepted"@en ;
    skos:definition "Measures associated with topics typically considered to be part of 'Data Governance'"@en ;
    skos:prefLabel "Data Governance"@en .

dpv-owl:DataImporter a rdfs:Class,
        owl:Class ;
    dct:contributor "David Hickey, Georg P. Krog, Paul Ryan, Harshvardhan J. Pandit" ;
    dct:created "2021-09-08"^^xsd:date ;
    dct:source [ a schema:WebPage ;
            schema:name "EDPB Recommendations 01/2020 on Data Transfers" ;
            schema:url "https://edpb.europa.eu/our-work-tools/our-documents/recommendations/recommendations-012020-measures-supplement-transfer_en" ] ;
    vann:example dex-owl:E0035 ;
    rdfs:isDefinedBy dpv-owl: ;
    rdfs:subClassOf dpv-owl:Recipient ;
    sw:term_status "accepted"@en ;
    skos:definition "An entity that 'imports' data where importing is considered a form of data transfer"@en ;
    skos:prefLabel "Data Importer"@en ;
    skos:scopeNote "The term 'Data Importer' is used by the EU-EDPB as the entity that receives transferred data across borders. While the EDPB refers to the jurisdictional border of EU, the term within DPV can be used to denote any 'import' or reception of transfer or transmission of data and is thus a broader concept than the EDPB's definition."@en .

dpv-owl:DataInteroperabilityAssessment a rdfs:Class,
        owl:Class,
        dpv-owl:OrganisationalMeasure ;
    dct:contributor "Harshvardhan J. Pandit" ;
    dct:created "2024-04-14"^^xsd:date ;
    rdfs:isDefinedBy dpv-owl: ;
    rdfs:subClassOf dpv-owl:Assessment,
        dpv-owl:DataInteroperabilityManagement ;
    sw:term_status "accepted"@en ;
    skos:definition "Measures associated with assessment of data interoperability"@en ;
    skos:prefLabel "Data Interoperability Assessment"@en .

dpv-owl:DataInteroperabilityImprovement a rdfs:Class,
        owl:Class,
        dpv-owl:OrganisationalMeasure ;
    dct:contributor "Beatriz Esteves, Harshvardhan J. Pandit" ;
    dct:created "2024-04-14"^^xsd:date ;
    dct:source "DGA 12.d"@en ;
    rdfs:isDefinedBy dpv-owl: ;
    rdfs:subClassOf dpv-owl:DataInteroperabilityManagement ;
    sw:term_status "accepted"@en ;
    skos:definition "Measures associated with improvement of data interoperability"@en ;
    skos:prefLabel "Data Interoperability Improvement"@en .

dpv-owl:DataInteroperabilityManagement a rdfs:Class,
        owl:Class,
        dpv-owl:OrganisationalMeasure ;
    dct:contributor "Harshvardhan J. Pandit" ;
    dct:created "2024-04-14"^^xsd:date ;
    rdfs:isDefinedBy dpv-owl: ;
    rdfs:subClassOf dpv-owl:DataGovernance ;
    sw:term_status "accepted"@en ;
    skos:definition "Measures associated with management of data interoperability"@en ;
    skos:prefLabel "Data Interoperability Management"@en .

dpv-owl:DataInventoryManagement a rdfs:Class,
        owl:Class,
        dpv-owl:OrganisationalMeasure ;
    dct:contributor "Harshvardhan J. Pandit" ;
    dct:created "2024-04-14"^^xsd:date ;
    rdfs:isDefinedBy dpv-owl: ;
    rdfs:subClassOf dpv-owl:DataGovernance ;
    sw:term_status "accepted"@en ;
    skos:definition "Measures associated with management of data inventory or a data asset list"@en ;
    skos:prefLabel "Data Inventory Management"@en .

dpv-owl:DataJurisdictionPolicy a rdfs:Class,
        owl:Class,
        dpv-owl:OrganisationalMeasure ;
    dct:contributor "Harshvardhan J. Pandit" ;
    dct:created "2024-04-14"^^xsd:date ;
    rdfs:isDefinedBy dpv-owl: ;
    rdfs:subClassOf dpv-owl:DataProcessingPolicy ;
    sw:term_status "accepted"@en ;
    skos:definition "Policy specifying jurisdictional requirements for data processing"@en ;
    skos:prefLabel "Data Jurisdiction Policy"@en ;
    skos:scopeNote "Jurisdictional requirements can refer to data being stored within specific jurisdictions, or that data must be in line with jurisdictional laws and norms"@en .

dpv-owl:DataLiteracy a rdfs:Class,
        owl:Class,
        dpv-owl:OrganisationalMeasure ;
    dct:contributor "Harshvardhan J. Pandit" ;
    dct:created "2024-05-17"^^xsd:date ;
    rdfs:isDefinedBy dpv-owl: ;
    rdfs:subClassOf dpv-owl:DigitalLiteracy ;
    sw:term_status "accepted"@en ;
    skos:definition "Providing skills, knowledge, and understanding to enable reading, writing, analysing, reasoning, and communicating regarding data"@en ;
    skos:prefLabel "Data Literacy"@en .

dpv-owl:DataProcessingAgreement a rdfs:Class,
        owl:Class,
        dpv-owl:LegalMeasure ;
    dct:contributor "Georg P. Krog, Harshvardhan J. Pandit, Beatriz Esteves, Paul Ryan, Julian Flake" ;
    dct:created "2022-01-26"^^xsd:date ;
    rdfs:isDefinedBy dpv-owl: ;
    rdfs:subClassOf dpv-owl:LegalAgreement ;
    sw:term_status "accepted"@en ;
    skos:definition "An agreement outlining conditions, criteria, obligations, responsibilities, and specifics for carrying out processing of data"@en ;
    skos:prefLabel "Data Processing Agreement"@en ;
    skos:scopeNote "For specific role-based data processing agreements, see concepts for Processors and JointDataController agreements."@en .

dpv-owl:DataProcessingPolicy a rdfs:Class,
        owl:Class,
        dpv-owl:OrganisationalMeasure ;
    dct:contributor "Harshvardhan J. Pandit" ;
    dct:created "2024-04-14"^^xsd:date ;
    rdfs:isDefinedBy dpv-owl: ;
    rdfs:subClassOf dpv-owl:Policy ;
    sw:term_status "accepted"@en ;
    skos:definition "Policy regarding data processing activities"@en ;
    skos:prefLabel "Data Processing Policy"@en ;
    skos:scopeNote "This only refers to the policy or plan or procedure describing how the data processing should be conducted. To represent the granular details, see further concepts e.g. dpv:DataStoragePolicy to describe policy regarding storage, or dpv:DataStorageCondition to represent information within the policy for how information should be stored"@en .

dpv-owl:DataProcessingRecord a rdfs:Class,
        owl:Class,
        dpv-owl:OrganisationalMeasure ;
    dct:contributor "Harshvardhan J. Pandit" ;
    dct:created "2021-09-08"^^xsd:date ;
    rdfs:isDefinedBy dpv-owl: ;
    rdfs:subClassOf dpv-owl:RecordsOfActivities ;
    sw:term_status "accepted"@en ;
    skos:definition "Record of data processing, whether ex-ante or ex-post"@en ;
    skos:prefLabel "Data Processing Record"@en .

dpv-owl:DataProcessor a rdfs:Class,
        owl:Class ;
    dct:contributor "Harshvardhan J. Pandit" ;
    dct:created "2019-06-04"^^xsd:date ;
    dct:source [ a schema:WebPage ;
            schema:name "GDPR Art.4-8" ;
            schema:url "https://eur-lex.europa.eu/eli/reg/2016/679/art_4/par_8/oj" ] ;
    vann:example dex-owl:E0033 ;
    rdfs:isDefinedBy dpv-owl: ;
    rdfs:subClassOf dpv-owl:Recipient ;
    sw:term_status "accepted"@en ;
    skos:definition "A ‘processor’ means a natural or legal person, public authority, agency or other body which processes data on behalf of the controller."@en ;
    skos:prefLabel "Data Processor"@en .

dpv-owl:DataProcessorContract a rdfs:Class,
        owl:Class,
        dpv-owl:LegalBasis ;
    dct:created "2023-12-10"^^xsd:date ;
    rdfs:isDefinedBy dpv-owl: ;
    rdfs:subClassOf dpv-owl:Contract ;
    sw:term_status "accepted"@en ;
    skos:definition "Creation, completion, fulfilment, or performance of a contract, with the Data Controller and Data Processor as parties, and involving specified processing of data or technologies"@en ;
    skos:prefLabel "Data Processor Contract"@en .

dpv-owl:DataProtectionAuthority a rdfs:Class,
        owl:Class ;
    dct:contributor "Georg P. Krog, Paul Ryan, Harshvardhan J. Pandit" ;
    dct:created "2020-11-04"^^xsd:date ;
    vann:example dex-owl:E0036 ;
    rdfs:isDefinedBy dpv-owl: ;
    rdfs:subClassOf dpv-owl:Authority ;
    sw:term_status "accepted"@en ;
    skos:definition "An authority tasked with overseeing legal compliance regarding privacy and data protection laws."@en ;
    skos:prefLabel "Data Protection Authority"@en .

dpv-owl:DataProtectionOfficer a rdfs:Class,
        owl:Class ;
    dct:contributor "Georg P. Krog, Paul Ryan" ;
    dct:created "2020-11-04"^^xsd:date ;
    dct:modified "2021-12-08"^^xsd:date ;
    dct:source [ a schema:WebPage ;
            schema:name "GDPR Art.37" ;
            schema:url "https://eur-lex.europa.eu/eli/reg/2016/679/art_37/oj" ] ;
    rdfs:isDefinedBy dpv-owl: ;
    rdfs:subClassOf dpv-owl:Representative ;
    sw:term_status "accepted"@en ;
    skos:definition "An entity within or authorised by an organisation to monitor internal compliance, inform and advise on data protection obligations and act as a contact point for data subjects and the supervisory authority."@en ;
    skos:prefLabel "Data Protection Officer"@en .

dpv-owl:DataProtectionTraining a rdfs:Class,
        owl:Class,
        dpv-owl:OrganisationalMeasure ;
    dct:contributor "Harshvardhan J. Pandit" ;
    dct:created "2022-08-17"^^xsd:date ;
    dct:source [ a schema:WebPage ;
            schema:name "ENISA 5G Cybersecurity Standards" ;
            schema:url "https://www.enisa.europa.eu/publications/5g-cybersecurity-standards" ] ;
    rdfs:isDefinedBy dpv-owl: ;
    rdfs:subClassOf dpv-owl:StaffTraining ;
    sw:term_status "accepted"@en ;
    skos:definition "Training intended to increase knowledge regarding data protection"@en ;
    skos:prefLabel "Data Protection Training"@en .

dpv-owl:DataPublishedByDataSubject a rdfs:Class,
        owl:Class,
        dpv-owl:DataSubjectDataSource ;
    dct:contributor "Julian Flake" ;
    dct:created "2022-08-24"^^xsd:date ;
    dct:modified "2023-12-10"^^xsd:date ;
    rdfs:isDefinedBy dpv-owl: ;
    rdfs:subClassOf dpv-owl:DataSubjectDataSource ;
    sw:term_status "accepted"@en ;
    skos:definition "Data is published by the data subject"@en ;
    skos:prefLabel "Data published by Data Subject"@en ;
    skos:scopeNote "This refers to where that data was made publicly available by the data subject. An example of this would be a social media profile that the data subject has made publicly accessible."@en .

dpv-owl:DataQualityAssessment a rdfs:Class,
        owl:Class,
        dpv-owl:OrganisationalMeasure ;
    dct:contributor "Harshvardhan J. Pandit" ;
    dct:created "2024-04-14"^^xsd:date ;
    rdfs:isDefinedBy dpv-owl: ;
    rdfs:subClassOf dpv-owl:Assessment,
        dpv-owl:DataQualityManagement ;
    sw:term_status "accepted"@en ;
    skos:definition "Measures associated with assessment of data quality"@en ;
    skos:prefLabel "Data Quality Assessment"@en .

dpv-owl:DataQualityImprovement a rdfs:Class,
        owl:Class,
        dpv-owl:OrganisationalMeasure ;
    dct:contributor "Harshvardhan J. Pandit" ;
    dct:created "2024-04-14"^^xsd:date ;
    rdfs:isDefinedBy dpv-owl: ;
    rdfs:subClassOf dpv-owl:DataQualityManagement ;
    sw:term_status "accepted"@en ;
    skos:definition "Measures associated with improvement of data quality"@en ;
    skos:prefLabel "Data Quality Improvement"@en .

dpv-owl:DataQualityManagement a rdfs:Class,
        owl:Class,
        dpv-owl:OrganisationalMeasure ;
    dct:contributor "Harshvardhan J. Pandit" ;
    dct:created "2024-04-14"^^xsd:date ;
    rdfs:isDefinedBy dpv-owl: ;
    rdfs:subClassOf dpv-owl:DataGovernance ;
    sw:term_status "accepted"@en ;
    skos:definition "Measures associated with management of data quality"@en ;
    skos:prefLabel "Data Quality Management"@en .

dpv-owl:DataRedaction a rdfs:Class,
        owl:Class,
        dpv-owl:TechnicalMeasure ;
    dct:contributor "Harshvardhan J. Pandit" ;
    dct:created "2020-10-01"^^xsd:date ;
    rdfs:isDefinedBy dpv-owl: ;
    rdfs:subClassOf dpv-owl:DataSanitisationTechnique ;
    sw:term_status "accepted"@en ;
    skos:definition "Removal of sensitive information from a data or document"@en ;
    skos:prefLabel "Data Redaction"@en .

dpv-owl:DataRestorationPolicy a rdfs:Class,
        owl:Class,
        dpv-owl:OrganisationalMeasure ;
    dct:contributor "Georg P. Krog, Harshvardhan J. Pandit" ;
    dct:created "2024-04-14"^^xsd:date ;
    rdfs:isDefinedBy dpv-owl: ;
    rdfs:subClassOf dpv-owl:DataProcessingPolicy ;
    sw:term_status "accepted"@en ;
    skos:definition "Policy regarding restoration of data"@en ;
    skos:prefLabel "Data Restoration Policy"@en ;
    skos:scopeNote "Restoration can refer to how data is restored from a backup"@en .

dpv-owl:DataReusePolicy a rdfs:Class,
        owl:Class,
        dpv-owl:OrganisationalMeasure ;
    dct:contributor "Harshvardhan J. Pandit" ;
    dct:created "2024-04-14"^^xsd:date ;
    rdfs:isDefinedBy dpv-owl: ;
    rdfs:subClassOf dpv-owl:DataProcessingPolicy ;
    sw:term_status "accepted"@en ;
    skos:definition "Policy regarding reuse of data i.e. using data for purposes other than its initial purpose"@en ;
    skos:prefLabel "Data Reuse Policy"@en ;
    skos:scopeNote "This policy can be used to describe the procedures associated with undertaking such reuse of data, for example to assess its legality and the compatibility of the initial and subsequent purposes"@en .

dpv-owl:DataSanitisationTechnique a rdfs:Class,
        owl:Class,
        dpv-owl:TechnicalMeasure ;
    dct:contributor "Harshvardhan J. Pandit" ;
    dct:created "2022-08-17"^^xsd:date ;
    dct:source [ a schema:WebPage ;
            schema:name "ENISA Reference Incident Classification Taxonomy 2018" ;
            schema:url "https://www.enisa.europa.eu/publications/reference-incident-classification-taxonomy/" ] ;
    rdfs:isDefinedBy dpv-owl: ;
    rdfs:subClassOf dpv-owl:TechnicalMeasure ;
    sw:term_status "accepted"@en ;
    skos:definition "Cleaning or any removal or re-organisation of elements in data based on selective criteria"@en ;
    skos:prefLabel "Data Sanitisation Technique"@en .

dpv-owl:DataSecurityManagement a rdfs:Class,
        owl:Class,
        dpv-owl:OrganisationalMeasure ;
    dct:contributor "Harshvardhan J. Pandit" ;
    dct:created "2024-04-14"^^xsd:date ;
    rdfs:isDefinedBy dpv-owl: ;
    rdfs:subClassOf dpv-owl:DataGovernance,
        dpv-owl:SecurityProcedure ;
    sw:term_status "accepted"@en ;
    skos:definition "Measures associated with management of data security"@en ;
    skos:prefLabel "Data Security Management"@en ;
    skos:scopeNote "Examples of data security management are assessing the appropriate security controls such as encryption, testing the implemented security controls, and ensuring it is protected and safeguarded from unintended actions"@en .

dpv-owl:DataSource a rdfs:Class,
        owl:Class ;
    dct:contributor "Georg P. Krog, Harshvardhan J. Pandit, Beatriz Esteves" ;
    dct:created "2020-11-04"^^xsd:date ;
    vann:example dex-owl:E0012 ;
    rdfs:isDefinedBy dpv-owl: ;
    rdfs:subClassOf dpv-owl:ProcessingContext ;
    sw:term_status "accepted"@en ;
    skos:definition "The source or origin of data"@en ;
    skos:prefLabel "Data Source"@en ;
    skos:scopeNote "Source' is the direct point of data collection; 'origin' would indicate the original/others points of where the data originates from."@en .

dpv-owl:DataStoragePolicy a rdfs:Class,
        owl:Class,
        dpv-owl:OrganisationalMeasure ;
    dct:contributor "Georg P. Krog, Harshvardhan J. Pandit" ;
    dct:created "2024-04-14"^^xsd:date ;
    rdfs:isDefinedBy dpv-owl: ;
    rdfs:subClassOf dpv-owl:DataProcessingPolicy ;
    sw:term_status "accepted"@en ;
    skos:definition "Policy regarding storage of data, including the manner, duration, location, and conditions for storage"@en ;
    skos:prefLabel "Data Storage Policy"@en .

dpv-owl:DataSubProcessor a rdfs:Class,
        owl:Class ;
    dct:contributor "Harshvardhan J. Pandit" ;
    dct:created "2020-11-25"^^xsd:date ;
    rdfs:isDefinedBy dpv-owl: ;
    rdfs:subClassOf dpv-owl:DataProcessor ;
    sw:term_status "accepted"@en ;
    skos:definition "A 'sub-processor' is a processor engaged by another processor"@en ;
    skos:prefLabel "Data Sub-Processor"@en ;
    skos:scopeNote "A 'Sub-Processor' is always a 'Processor' with the distinction of not directly being appointed by the 'Controller'"@en .

dpv-owl:DataSubject a rdfs:Class,
        owl:Class ;
    dct:contributor "Axel Polleres, Javier Fernández" ;
    dct:created "2019-04-05"^^xsd:date ;
    dct:modified "2020-11-04"^^xsd:date ;
    dct:source [ a schema:WebPage ;
            schema:name "GDPR Art.4-1g" ;
            schema:url "https://eur-lex.europa.eu/eli/reg/2016/679/art_4/par_1/oj" ] ;
    vann:example dex-owl:E0039 ;
    rdfs:isDefinedBy dpv-owl: ;
    rdfs:subClassOf dpv-owl:LegalEntity ;
    sw:term_status "accepted"@en ;
    skos:definition "The individual (or category of individuals) whose personal data is being processed"@en ;
    skos:prefLabel "Data Subject"@en ;
    skos:scopeNote "The term 'data subject' is specific to the GDPR, but is functionally equivalent to the term 'individual associated with data' and the ISO/IEC term 'PII Principle'"@en .

dpv-owl:DataSubjectContract a rdfs:Class,
        owl:Class,
        dpv-owl:LegalBasis ;
    dct:created "2023-12-10"^^xsd:date ;
    rdfs:isDefinedBy dpv-owl: ;
    rdfs:subClassOf dpv-owl:Contract ;
    sw:term_status "accepted"@en ;
    skos:definition "Creation, completion, fulfilment, or performance of a contract, with the Data Controller and Data Subject as parties, and involving specified processing of data or technologies"@en ;
    skos:prefLabel "Data Subject Contract"@en .

dpv-owl:DataSubjectDataSource a rdfs:Class,
        owl:Class,
        dpv-owl:DataSource ;
    dct:created "2023-10-12"^^xsd:date ;
    rdfs:isDefinedBy dpv-owl: ;
    rdfs:subClassOf dpv-owl:DataSource ;
    sw:term_status "accepted"@en ;
    skos:definition "Data Sourced from Data Subject(s), e.g. when data is collected via a form or observed from their activities"@en ;
    skos:prefLabel "Data Subject as Data Source"@en .

dpv-owl:DataSubjectInformed a rdfs:Class,
        owl:Class,
        dpv-owl:EntityInformedStatus ;
    dct:contributor "Harshvardhan J. Pandit, Delaram Golpayegani, Georg P. Krog, Paul Ryan" ;
    dct:created "2024-05-10"^^xsd:date ;
    rdfs:isDefinedBy dpv-owl: ;
    rdfs:subClassOf dpv-owl:EntityInformed ;
    sw:term_status "accepted"@en ;
    skos:definition "Status indicating DataSubject has been informed about the specified context"@en ;
    skos:prefLabel "Data Subject Informed"@en .

dpv-owl:DataSubjectRight a rdfs:Class,
        owl:Class,
        dpv-owl:Right ;
    dct:contributor "Beatriz Esteves, Georg P. Krog, Harshvardhan J. Pandit" ;
    dct:created "2020-11-18"^^xsd:date ;
    rdfs:isDefinedBy dpv-owl: ;
    rdfs:subClassOf dpv-owl:Right ;
    sw:term_status "accepted"@en ;
    skos:definition "The rights applicable or provided to a Data Subject"@en ;
    skos:prefLabel "Data Subject Right"@en ;
    skos:scopeNote "Based on use of definitions, the notion of 'Data Subject Right' can be equivalent to 'Individual Right' or 'Right of a Person'"@en .

dpv-owl:DataSubjectRightsManagement a rdfs:Class,
        owl:Class,
        dpv-owl:OrganisationalMeasure ;
    dct:contributor "Beatriz Esteves, Harshvardhan J. Pandit, Georg P. Krog" ;
    dct:created "2024-04-14"^^xsd:date ;
    dct:source "DGA 12.m"@en ;
    rdfs:isDefinedBy dpv-owl: ;
    rdfs:subClassOf dpv-owl:RightsManagement ;
    sw:term_status "accepted"@en ;
    skos:definition "Methods to provide, implement, and exercise data subjects' rights"@en ;
    skos:prefLabel "Data Subject Rights Management"@en ;
    skos:scopeNote "This concept only concerns the organisational management of rights, and does not represent the rights themselves - especially where such 'rights' are legally recognised or defined for the data subject or individual. The concept dpv:DataSubjectRight is provided to represent such legal rights."@en .

dpv-owl:DataSubjectScale a rdfs:Class,
        owl:Class ;
    dct:contributor "Harshvardhan J. Pandit, Georg P. Krog, Rana Saniei" ;
    dct:created "2022-06-15"^^xsd:date ;
    vann:example dex-owl:E0049 ;
    rdfs:isDefinedBy dpv-owl: ;
    rdfs:subClassOf dpv-owl:Scale ;
    sw:term_status "accepted"@en ;
    skos:definition "Scale of Data Subject(s)"@en ;
    skos:prefLabel "Data Subject Scale"@en .

dpv-owl:DataSubjectUninformed a rdfs:Class,
        owl:Class,
        dpv-owl:EntityInformedStatus ;
    dct:contributor "Harshvardhan J. Pandit, Delaram Golpayegani, Georg P. Krog, Paul Ryan" ;
    dct:created "2024-05-10"^^xsd:date ;
    rdfs:isDefinedBy dpv-owl: ;
    rdfs:subClassOf dpv-owl:EntityUninformed ;
    sw:term_status "accepted"@en ;
    skos:definition "Status indicating DataSubject is uninformed i.e. has not been informed about the specified context"@en ;
    skos:prefLabel "Data Subject Uninformed"@en .

dpv-owl:DataTransferImpactAssessment a rdfs:Class,
        owl:Class,
        dpv-owl:OrganisationalMeasure ;
    dct:contributor "Georg P. Krog, Harshvardhan J. Pandit, Paul Ryan" ;
    dct:created "2021-09-08"^^xsd:date ;
    rdfs:isDefinedBy dpv-owl: ;
    rdfs:subClassOf dpv-owl:ImpactAssessment ;
    sw:term_status "accepted"@en ;
    skos:definition "Impact Assessment for conducting data transfers"@en ;
    skos:prefLabel "Data Transfer Impact Assessment"@en .

dpv-owl:DataTransferLegalBasis a rdfs:Class,
        owl:Class,
        dpv-owl:LegalBasis ;
    dct:contributor "David Hickey, Georg P. Krog" ;
    dct:created "2021-09-08"^^xsd:date ;
    rdfs:isDefinedBy dpv-owl: ;
    rdfs:subClassOf dpv-owl:LegalBasis ;
    sw:term_status "accepted"@en ;
    skos:definition "Specific or special categories and instances of legal basis intended for justifying data transfers"@en ;
    skos:prefLabel "Data Transfer Legal Basis"@en .

dpv-owl:DataTransferNotice a rdfs:Class,
        owl:Class,
        dpv-owl:OrganisationalMeasure ;
    dct:contributor "Georg P. Krog, Paul Ryan, David Hickey, Beatriz Esteves, Harshvardhan J. Pandit" ;
    dct:created "2024-04-14"^^xsd:date ;
    dct:source "DGA 5.9"@en ;
    rdfs:isDefinedBy dpv-owl: ;
    rdfs:subClassOf dpv-owl:Notice ;
    sw:term_status "accepted"@en ;
    skos:definition "Notice for the legal entity for the transfer of its data"@en ;
    skos:prefLabel "Data Transfer Notice"@en .

dpv-owl:DataTransferRecord a rdfs:Class,
        owl:Class,
        dpv-owl:OrganisationalMeasure ;
    dct:contributor "Harshvardhan J. Pandit" ;
    dct:created "2024-04-14"^^xsd:date ;
    rdfs:isDefinedBy dpv-owl: ;
    rdfs:subClassOf dpv-owl:DataProcessingRecord ;
    sw:term_status "accepted"@en ;
    skos:definition "Record of data transfer activities"@en ;
    skos:prefLabel "Data Transfer Record"@en .

dpv-owl:DataVolume a rdfs:Class,
        owl:Class ;
    dct:contributor "Harshvardhan J. Pandit, Georg P. Krog, Rana Saniei" ;
    dct:created "2022-06-15"^^xsd:date ;
    vann:example dex-owl:E0049 ;
    rdfs:isDefinedBy dpv-owl: ;
    rdfs:subClassOf dpv-owl:Scale ;
    sw:term_status "accepted"@en ;
    skos:definition "Volume or Scale of Data"@en ;
    skos:prefLabel "Data Volume"@en .

dpv-owl:DecentralisedLocations a rdfs:Class,
        owl:Class,
        dpv-owl:LocationFixture ;
    dct:contributor "Harshvardhan J. Pandit" ;
    dct:created "2022-06-15"^^xsd:date ;
    dct:modified "2020-10-05"^^xsd:date ;
    rdfs:isDefinedBy dpv-owl: ;
    rdfs:subClassOf dpv-owl:LocationFixture ;
    sw:term_status "accepted"@en ;
    skos:definition "Location that is spread across multiple separate areas with no distinction between their importance"@en ;
    skos:prefLabel "Decentralised Locations"@en .

dpv-owl:DecisionMaking a rdfs:Class,
        owl:Class ;
    dct:contributor "Harshvardhan J. Pandit" ;
    dct:created "2022-09-07"^^xsd:date ;
    rdfs:isDefinedBy dpv-owl: ;
    rdfs:subClassOf dpv-owl:ProcessingContext ;
    sw:term_status "accepted"@en ;
    skos:definition "Processing that involves decision making"@en ;
    skos:prefLabel "Decision Making"@en .

dpv-owl:Deidentification a rdfs:Class,
        owl:Class,
        dpv-owl:TechnicalMeasure ;
    dct:contributor "Axel Polleres, Rob Brennan, Harshvardhan J. Pandit, Mark Lizar" ;
    dct:created "2019-04-05"^^xsd:date ;
    dct:modified "2022-11-24"^^xsd:date ;
    dct:source [ a schema:WebPage ;
            schema:name "NISTIR 8053" ;
            schema:url "https://nvlpubs.nist.gov/nistpubs/ir/2015/NIST.IR.8053.pdf" ] ;
    rdfs:isDefinedBy dpv-owl: ;
    rdfs:subClassOf dpv-owl:DataSanitisationTechnique ;
    sw:term_status "accepted"@en ;
    skos:definition "Removal of identity or information to reduce identifiability"@en ;
    skos:prefLabel "De-Identification"@en .

dpv-owl:Delete a rdfs:Class,
        owl:Class,
        dpv-owl:Processing ;
    dct:contributor "Harshvardhan J. Pandit" ;
    dct:created "2024-04-14"^^xsd:date ;
    rdfs:isDefinedBy dpv-owl: ;
    rdfs:subClassOf dpv-owl:Remove ;
    sw:term_status "accepted"@en ;
    skos:definition "to remove data in a logical fashion i.e. with the possibility of retrieval"@en ;
    skos:prefLabel "Delete"@en .

dpv-owl:DeliveryOfGoods a rdfs:Class,
        owl:Class,
        dpv-owl:Purpose ;
    dct:contributor "Harshvardhan J. Pandit, Javier Fernández, Axel Polleres, Elmar Kiesling, Fajar Ekaputra, Simon Steyskal" ;
    dct:created "2019-04-05"^^xsd:date ;
    rdfs:isDefinedBy dpv-owl: ;
    rdfs:subClassOf dpv-owl:RequestedServiceProvision ;
    sw:term_status "accepted"@en ;
    skos:definition "Purposes associated with delivering goods and services requested or asked by consumer"@en ;
    skos:prefLabel "Delivery of Goods"@en ;
    skos:related svpu:Delivery .

dpv-owl:Derive a rdfs:Class,
        owl:Class,
        dpv-owl:Processing ;
    dct:created "2019-05-07"^^xsd:date ;
    dct:source [ a schema:WebPage ;
            schema:name "SPECIAL Project" ;
            schema:url "https://specialprivacy.ercim.eu/vocabs/processing" ] ;
    vann:example dex-owl:E0009 ;
    rdfs:isDefinedBy dpv-owl: ;
    rdfs:subClassOf dpv-owl:Obtain ;
    sw:term_status "accepted"@en ;
    skos:definition "to create new derivative data from the original data"@en ;
    skos:prefLabel "Derive"@en ;
    skos:related svpr:Derive ;
    skos:scopeNote "Derive indicates data is present or obtainable from existing data. For data that is created without such existence, see Infer."@en .

dpv-owl:DerivedData a rdfs:Class,
        owl:Class ;
    dct:created "2023-12-10"^^xsd:date ;
    rdfs:isDefinedBy dpv-owl: ;
    rdfs:subClassOf dpv-owl:Data ;
    sw:term_status "accepted"@en ;
    skos:definition "Data that has been obtained through derivations of other data"@en ;
    skos:prefLabel "Derived Data"@en .

dpv-owl:DerivedPersonalData a rdfs:Class,
        owl:Class ;
    dct:contributor "Elmar Kiesling; Harshvardhan J. Pandit, Fajar Ekaputra" ;
    dct:created "2019-05-07"^^xsd:date ;
    dct:modified "2023-12-10"^^xsd:date ;
    dct:source [ a schema:WebPage ;
            schema:name "DPVCG" ;
            schema:url "https://www.w3.org/community/dpvcg/" ] ;
    vann:example dex-owl:E0009,
        dex-owl:E0046 ;
    rdfs:isDefinedBy dpv-owl: ;
    rdfs:subClassOf dpv-owl:DerivedData,
        dpv-owl:PersonalData ;
    sw:term_status "accepted"@en ;
    skos:definition "Personal Data that is obtained or derived from other data"@en ;
    skos:prefLabel "Derived Personal Data"@en ;
    skos:related svd:Derived ;
    skos:scopeNote "Derived Data is data that is obtained through processing of existing data, e.g. deriving first name from full name. To indicate data that is derived but which was not present or evident within the source data, InferredPersonalData should be used."@en .

dpv-owl:DesignStandard a rdfs:Class,
        owl:Class,
        dpv-owl:OrganisationalMeasure ;
    dct:contributor "Axel Polleres, Rob Brennan, Harshvardhan J. Pandit, Mark Lizar" ;
    dct:created "2019-04-05"^^xsd:date ;
    rdfs:isDefinedBy dpv-owl: ;
    rdfs:subClassOf dpv-owl:GuidelinesPrinciple ;
    sw:term_status "accepted"@en ;
    skos:definition "A set of rules or guidelines outlining criterias for design"@en ;
    skos:prefLabel "Design Standard"@en .

dpv-owl:Destruct a rdfs:Class,
        owl:Class,
        dpv-owl:Processing ;
    dct:created "2019-05-07"^^xsd:date ;
    dct:source [ a schema:WebPage ;
            schema:name "GDPR Art.4-2" ;
            schema:url "https://eur-lex.europa.eu/eli/reg/2016/679/art_4/par_2/oj" ] ;
    rdfs:isDefinedBy dpv-owl: ;
    rdfs:subClassOf dpv-owl:Remove ;
    sw:term_status "accepted"@en ;
    skos:definition "to process data in a way it no longer exists or cannot be repaired"@en ;
    skos:prefLabel "Destruct"@en .

dpv-owl:DeterministicPseudonymisation a rdfs:Class,
        owl:Class,
        dpv-owl:TechnicalMeasure ;
    dct:contributor "Harshvardhan J. Pandit" ;
    dct:created "2022-08-17"^^xsd:date ;
    dct:source [ a schema:WebPage ;
            schema:name "ENISA Data Pseudonymisation: Advanced Techniques and Use Cases" ;
            schema:url "https://www.enisa.europa.eu/publications/data-pseudonymisation-advanced-techniques-and-use-cases" ] ;
    rdfs:isDefinedBy dpv-owl: ;
    rdfs:subClassOf dpv-owl:Pseudonymisation ;
    sw:term_status "accepted"@en ;
    skos:definition "Pseudonymisation achieved through a deterministic function"@en ;
    skos:prefLabel "Deterministic Pseudonymisation"@en .

dpv-owl:DifferentialPrivacy a rdfs:Class,
        owl:Class,
        dpv-owl:TechnicalMeasure ;
    dct:contributor "Harshvardhan J. Pandit" ;
    dct:created "2022-08-17"^^xsd:date ;
    dct:source [ a schema:WebPage ;
            schema:name "ENISA Data Protection Engineering" ;
            schema:url "https://www.enisa.europa.eu/publications/data-protection-engineering" ] ;
    rdfs:isDefinedBy dpv-owl: ;
    rdfs:subClassOf dpv-owl:CryptographicMethods ;
    sw:term_status "accepted"@en ;
    skos:definition "Utilisation of differential privacy where information is shared as patterns or groups to withhold individual elements"@en ;
    skos:prefLabel "Differential Privacy"@en .

dpv-owl:DigitalLiteracy a rdfs:Class,
        owl:Class,
        dpv-owl:OrganisationalMeasure ;
    dct:contributor "Harshvardhan J. Pandit" ;
    dct:created "2024-05-17"^^xsd:date ;
    rdfs:isDefinedBy dpv-owl: ;
    rdfs:subClassOf dpv-owl:OrganisationalMeasure ;
    sw:term_status "accepted"@en ;
    skos:definition "Providing skills, knowledge, and understanding to enable reading, writing, analysing, reasoning, and communicating regarding digital technologies and their implications"@en ;
    skos:prefLabel "Digital Literacy"@en .

dpv-owl:DigitalRightsManagement a rdfs:Class,
        owl:Class,
        dpv-owl:TechnicalMeasure ;
    dct:contributor "Harshvardhan J. Pandit" ;
    dct:created "2022-08-17"^^xsd:date ;
    dct:source [ a schema:WebPage ;
            schema:name "ENISA Reference Incident Classification Taxonomy 2018" ;
            schema:url "https://www.enisa.europa.eu/publications/reference-incident-classification-taxonomy/" ] ;
    rdfs:isDefinedBy dpv-owl: ;
    rdfs:subClassOf dpv-owl:TechnicalMeasure ;
    sw:term_status "accepted"@en ;
    skos:definition "Management of access, use, and other operations associated with digital content"@en ;
    skos:prefLabel "Digital Rights Management"@en .

dpv-owl:DigitalSignatures a rdfs:Class,
        owl:Class,
        dpv-owl:TechnicalMeasure ;
    dct:contributor "Harshvardhan J. Pandit" ;
    dct:created "2022-08-17"^^xsd:date ;
    dct:source [ a schema:WebPage ;
            schema:name "ENISA Reference Incident Classification Taxonomy 2018" ;
            schema:url "https://www.enisa.europa.eu/publications/reference-incident-classification-taxonomy/" ] ;
    rdfs:isDefinedBy dpv-owl: ;
    rdfs:subClassOf dpv-owl:CryptographicMethods ;
    sw:term_status "accepted"@en ;
    skos:definition "Expression and authentication of identity through digital information containing cryptographic signatures"@en ;
    skos:prefLabel "Digital Signatures"@en .

dpv-owl:DirectMarketing a rdfs:Class,
        owl:Class,
        dpv-owl:Purpose ;
    dct:contributor "Georg P. Krog, Harshvardhan J. Pandit, Beatriz Esteves" ;
    dct:created "2020-11-04"^^xsd:date ;
    rdfs:isDefinedBy dpv-owl: ;
    rdfs:subClassOf dpv-owl:Marketing ;
    sw:term_status "accepted"@en ;
    skos:definition "Purposes associated with conducting direct marketing i.e. marketing communicated directly to the individual"@en ;
    skos:prefLabel "Direct Marketing"@en .

dpv-owl:DisasterRecoveryProcedures a rdfs:Class,
        owl:Class,
        dpv-owl:OrganisationalMeasure ;
    dct:contributor "Harshvardhan J. Pandit" ;
    dct:created "2022-08-17"^^xsd:date ;
    dct:source [ a schema:WebPage ;
            schema:name "ENISA 5G Cybersecurity Standards" ;
            schema:url "https://www.enisa.europa.eu/publications/5g-cybersecurity-standards" ] ;
    rdfs:isDefinedBy dpv-owl: ;
    rdfs:subClassOf dpv-owl:GovernanceProcedures ;
    sw:term_status "accepted"@en ;
    skos:definition "Procedures related to management of disasters and recovery"@en ;
    skos:prefLabel "Disaster Recovery Procedures"@en .

dpv-owl:Disclose a rdfs:Class,
        owl:Class,
        dpv-owl:Processing ;
    dct:created "2019-05-07"^^xsd:date ;
    dct:source [ a schema:WebPage ;
            schema:name "GDPR Art.4-2" ;
            schema:url "https://eur-lex.europa.eu/eli/reg/2016/679/art_4/par_2/oj" ] ;
    rdfs:isDefinedBy dpv-owl: ;
    rdfs:subClassOf dpv-owl:Processing ;
    sw:term_status "accepted"@en ;
    skos:definition "to make data known"@en ;
    skos:prefLabel "Disclose"@en .

dpv-owl:DiscloseByTransmission a rdfs:Class,
        owl:Class,
        dpv-owl:Processing ;
    dct:created "2019-05-07"^^xsd:date ;
    dct:source [ a schema:WebPage ;
            schema:name "GDPR Art.4-2" ;
            schema:url "https://eur-lex.europa.eu/eli/reg/2016/679/art_4/par_2/oj" ] ;
    rdfs:isDefinedBy dpv-owl: ;
    rdfs:subClassOf dpv-owl:Disclose ;
    sw:term_status "accepted"@en ;
    skos:definition "to disclose data by means of transmission"@en ;
    skos:prefLabel "Disclose by Transmission"@en .

dpv-owl:Display a rdfs:Class,
        owl:Class,
        dpv-owl:Processing ;
    dct:contributor "Beatriz Esteves" ;
    dct:created "2024-04-14"^^xsd:date ;
    dct:source "DGA 2.20"@en ;
    rdfs:isDefinedBy dpv-owl: ;
    rdfs:subClassOf dpv-owl:Disclose ;
    sw:term_status "accepted"@en ;
    skos:definition "to present or show data"@en ;
    skos:prefLabel "Display"@en .

dpv-owl:DisputeManagement a rdfs:Class,
        owl:Class,
        dpv-owl:Purpose ;
    dct:contributor "Georg P. Krog, Harshvardhan J. Pandit, Beatriz Esteves" ;
    dct:created "2021-09-08"^^xsd:date ;
    dct:source [ a schema:WebPage ;
            schema:name "Belgian DPA ROPA Template" ;
            schema:url "https://www.privacycommission.be/nl/model-voor-een-register-van-de-verwerkingsactiviteiten" ] ;
    rdfs:isDefinedBy dpv-owl: ;
    rdfs:subClassOf dpv-owl:OrganisationGovernance ;
    sw:term_status "accepted"@en ;
    skos:definition "Purposes associated with activities that manage disputes by natural persons, private bodies, or public authorities relevant to organisation"@en ;
    skos:prefLabel "Dispute Management"@en .

dpv-owl:Disseminate a rdfs:Class,
        owl:Class,
        dpv-owl:Processing ;
    dct:created "2019-05-07"^^xsd:date ;
    dct:source [ a schema:WebPage ;
            schema:name "GDPR Art.4-2" ;
            schema:url "https://eur-lex.europa.eu/eli/reg/2016/679/art_4/par_2/oj" ] ;
    rdfs:isDefinedBy dpv-owl: ;
    rdfs:subClassOf dpv-owl:Disclose ;
    sw:term_status "accepted"@en ;
    skos:definition "to spread data throughout"@en ;
    skos:prefLabel "Disseminate"@en .

dpv-owl:DistributedSystemSecurity a rdfs:Class,
        owl:Class,
        dpv-owl:TechnicalMeasure ;
    dct:contributor "Harshvardhan J. Pandit" ;
    dct:created "2022-08-17"^^xsd:date ;
    dct:source [ a schema:WebPage ;
            schema:name "ENISA Reference Incident Classification Taxonomy 2018" ;
            schema:url "https://www.enisa.europa.eu/publications/reference-incident-classification-taxonomy/" ] ;
    rdfs:isDefinedBy dpv-owl: ;
    rdfs:subClassOf dpv-owl:SecurityMethod ;
    sw:term_status "accepted"@en ;
    skos:definition "Security implementations provided using or over a distributed system"@en ;
    skos:prefLabel "Distributed System Security"@en .

dpv-owl:DocumentRandomisedPseudonymisation a rdfs:Class,
        owl:Class,
        dpv-owl:TechnicalMeasure ;
    dct:contributor "Harshvardhan J. Pandit" ;
    dct:created "2022-08-17"^^xsd:date ;
    dct:source [ a schema:WebPage ;
            schema:name "ENISA Data Pseudonymisation: Advanced Techniques and Use Cases" ;
            schema:url "https://www.enisa.europa.eu/publications/data-pseudonymisation-advanced-techniques-and-use-cases" ] ;
    rdfs:isDefinedBy dpv-owl: ;
    rdfs:subClassOf dpv-owl:Pseudonymisation ;
    sw:term_status "accepted"@en ;
    skos:definition "Use of randomised pseudonymisation where the same elements are assigned different values in the same document or database"@en ;
    skos:prefLabel "Document Randomised Pseudonymisation"@en .

dpv-owl:DocumentSecurity a rdfs:Class,
        owl:Class,
        dpv-owl:TechnicalMeasure ;
    dct:contributor "Harshvardhan J. Pandit" ;
    dct:created "2022-08-17"^^xsd:date ;
    dct:source [ a schema:WebPage ;
            schema:name "ENISA Reference Incident Classification Taxonomy 2018" ;
            schema:url "https://www.enisa.europa.eu/publications/reference-incident-classification-taxonomy/" ] ;
    rdfs:isDefinedBy dpv-owl: ;
    rdfs:subClassOf dpv-owl:SecurityMethod ;
    sw:term_status "accepted"@en ;
    skos:definition "Security measures enacted over documents to protect against tampering or restrict access"@en ;
    skos:prefLabel "Document Security"@en .

dpv-owl:Download a rdfs:Class,
        owl:Class,
        dpv-owl:Processing ;
    dct:contributor "Beatriz Esteves" ;
    dct:created "2024-04-14"^^xsd:date ;
    dct:source " 2.20"@en,
        "DGA 2.13"@en ;
    rdfs:isDefinedBy dpv-owl: ;
    rdfs:subClassOf dpv-owl:Disclose ;
    sw:term_status "accepted"@en ;
    skos:definition "to provide a copy or to receive a copy of data over a network or internet"@en ;
    skos:prefLabel "Download"@en .

dpv-owl:Duration a rdfs:Class,
        owl:Class ;
    dct:contributor "Harshvardhan J. Pandit" ;
    dct:created "2022-02-09"^^xsd:date ;
    vann:example dex-owl:E0050,
        dex-owl:E0070 ;
    rdfs:isDefinedBy dpv-owl: ;
    rdfs:subClassOf dpv-owl:Context ;
    sw:term_status "accepted"@en ;
    skos:definition "The duration or temporal limitation"@en ;
    skos:prefLabel "Duration"@en .

dpv-owl:EconomicUnion a rdfs:Class,
        owl:Class ;
    dct:contributor "Harshvardhan J. Pandit" ;
    dct:created "2022-01-19"^^xsd:date ;
    rdfs:isDefinedBy dpv-owl: ;
    rdfs:subClassOf dpv-owl:Location ;
    sw:term_status "accepted"@en ;
    skos:definition "A political union of two or more countries based on economic or trade agreements"@en ;
    skos:prefLabel "Economic Union"@en .

dpv-owl:EducationalTraining a rdfs:Class,
        owl:Class,
        dpv-owl:OrganisationalMeasure ;
    dct:contributor "Harshvardhan J. Pandit" ;
    dct:created "2022-08-17"^^xsd:date ;
    dct:source [ a schema:WebPage ;
            schema:name "ENISA Reference Incident Classification Taxonomy 2018" ;
            schema:url "https://www.enisa.europa.eu/publications/reference-incident-classification-taxonomy/" ] ;
    rdfs:isDefinedBy dpv-owl: ;
    rdfs:subClassOf dpv-owl:StaffTraining ;
    sw:term_status "accepted"@en ;
    skos:definition "Training methods that are intended to provide education on topic(s)"@en ;
    skos:prefLabel "Educational Training"@en .

dpv-owl:EffectivenessDeterminationProcedures a rdfs:Class,
        owl:Class,
        dpv-owl:OrganisationalMeasure ;
    dct:contributor "Harshvardhan J. Pandit" ;
    dct:created "2022-08-17"^^xsd:date ;
    dct:source [ a schema:WebPage ;
            schema:name "ENISA 5G Cybersecurity Standards" ;
            schema:url "https://www.enisa.europa.eu/publications/5g-cybersecurity-standards" ] ;
    rdfs:isDefinedBy dpv-owl: ;
    rdfs:subClassOf dpv-owl:Assessment ;
    sw:term_status "accepted"@en ;
    skos:definition "Procedures intended to determine effectiveness of other measures"@en ;
    skos:prefLabel "Effectiveness Determination Procedures"@en .

dpv-owl:ElderlyDataSubject a rdfs:Class,
        owl:Class,
        dpv-owl:DataSubject ;
    dct:contributor "Georg P. Krog" ;
    dct:created "2022-06-15"^^xsd:date ;
    rdfs:isDefinedBy dpv-owl: ;
    rdfs:subClassOf dpv-owl:VulnerableDataSubject ;
    sw:term_status "accepted"@en ;
    skos:definition "Data subjects that are considered elderly (i.e. based on age)"@en ;
    skos:prefLabel "Elderly Data Subject"@en .

dpv-owl:Employee a rdfs:Class,
        owl:Class,
        dpv-owl:DataSubject ;
    dct:contributor "Harshvardhan J. Pandit, Georg P. Krog, Julian Flake, Paul Ryan, Beatriz Esteves" ;
    dct:created "2022-04-06"^^xsd:date ;
    rdfs:isDefinedBy dpv-owl: ;
    rdfs:subClassOf dpv-owl:DataSubject ;
    sw:term_status "accepted"@en ;
    skos:definition "Data subjects that are employees"@en ;
    skos:prefLabel "Employee"@en .

dpv-owl:Encryption a rdfs:Class,
        owl:Class,
        dpv-owl:TechnicalMeasure ;
    dct:contributor "Axel Polleres, Rob Brennan, Harshvardhan J. Pandit, Mark Lizar" ;
    dct:created "2019-04-05"^^xsd:date ;
    vann:example dex-owl:E0020 ;
    rdfs:isDefinedBy dpv-owl: ;
    rdfs:subClassOf dpv-owl:TechnicalMeasure ;
    sw:term_status "accepted"@en ;
    skos:definition "Technical measures consisting of encryption"@en ;
    skos:prefLabel "Encryption"@en .

dpv-owl:EncryptionAtRest a rdfs:Class,
        owl:Class,
        dpv-owl:TechnicalMeasure ;
    dct:contributor "Axel Polleres, Rob Brennan, Harshvardhan J. Pandit, Mark Lizar" ;
    dct:created "2019-04-05"^^xsd:date ;
    rdfs:isDefinedBy dpv-owl: ;
    rdfs:subClassOf dpv-owl:Encryption ;
    sw:term_status "accepted"@en ;
    skos:definition "Encryption of data when being stored (persistent encryption)"@en ;
    skos:prefLabel "Encryption at Rest"@en .

dpv-owl:EncryptionInTransfer a rdfs:Class,
        owl:Class,
        dpv-owl:TechnicalMeasure ;
    dct:contributor "Axel Polleres, Rob Brennan, Harshvardhan J. Pandit, Mark Lizar" ;
    dct:created "2019-04-05"^^xsd:date ;
    rdfs:isDefinedBy dpv-owl: ;
    rdfs:subClassOf dpv-owl:Encryption ;
    sw:term_status "accepted"@en ;
    skos:definition "Encryption of data in transit e.g. when being transferred from one location to another, including sharing"@en ;
    skos:prefLabel "Encryption in Transfer"@en .

dpv-owl:EncryptionInUse a rdfs:Class,
        owl:Class,
        dpv-owl:TechnicalMeasure ;
    dct:contributor "Harshvardhan J. Pandit" ;
    dct:created "2022-10-22"^^xsd:date ;
    rdfs:isDefinedBy dpv-owl: ;
    rdfs:subClassOf dpv-owl:Encryption ;
    sw:term_status "accepted"@en ;
    skos:definition "Encryption of data when it is being used"@en ;
    skos:prefLabel "Encryption in Use"@en .

dpv-owl:EndToEndEncryption a rdfs:Class,
        owl:Class,
        dpv-owl:TechnicalMeasure ;
    dct:contributor "Harshvardhan J. Pandit" ;
    dct:created "2022-08-17"^^xsd:date ;
    dct:source [ a schema:WebPage ;
            schema:name "ENISA Data Protection Engineering" ;
            schema:url "https://www.enisa.europa.eu/publications/data-protection-engineering" ] ;
    rdfs:isDefinedBy dpv-owl: ;
    rdfs:subClassOf dpv-owl:Encryption ;
    sw:term_status "accepted"@en ;
    skos:definition "Encrypted communications where data is encrypted by the sender and decrypted by the intended receiver to prevent access to any third party"@en ;
    skos:prefLabel "End-to-End Encryption (E2EE)"@en .

dpv-owl:EndlessDuration a rdfs:Class,
        owl:Class,
        dpv-owl:Duration ;
    dct:contributor "Harshvardhan J. Pandit" ;
    dct:created "2022-06-15"^^xsd:date ;
    dct:modified "2020-10-05"^^xsd:date ;
    rdfs:isDefinedBy dpv-owl: ;
    rdfs:subClassOf dpv-owl:Duration ;
    sw:term_status "accepted"@en ;
    skos:definition "Duration that is (known or intended to be) open ended or without an end"@en ;
    skos:prefLabel "Endless Duration"@en .

dpv-owl:EnforceAccessControl a rdfs:Class,
        owl:Class,
        dpv-owl:Purpose ;
    dct:contributor "Harshvardhan J. Pandit, Javier Fernández, Axel Polleres, Elmar Kiesling, Fajar Ekaputra, Simon Steyskal" ;
    dct:created "2019-04-05"^^xsd:date ;
    rdfs:isDefinedBy dpv-owl: ;
    rdfs:subClassOf dpv-owl:EnforceSecurity ;
    sw:term_status "accepted"@en ;
    skos:definition "Purposes associated with conducting or enforcing access control as a form of security"@en ;
    skos:prefLabel "Enforce Access Control"@en ;
    skos:related svpu:Login ;
    skos:scopeNote "Was previously \"Access Control\". Prefixed to distinguish from Technical Measure."@en .

dpv-owl:EnforceSecurity a rdfs:Class,
        owl:Class,
        dpv-owl:Purpose ;
    dct:contributor "Harshvardhan J. Pandit, Javier Fernández, Axel Polleres, Elmar Kiesling, Fajar Ekaputra, Simon Steyskal" ;
    dct:created "2019-04-05"^^xsd:date ;
    rdfs:isDefinedBy dpv-owl: ;
    rdfs:subClassOf dpv-owl:Purpose ;
    sw:term_status "accepted"@en ;
    skos:definition "Purposes associated with ensuring and enforcing security for data, personnel, or other related matters"@en ;
    skos:prefLabel "Enforce Security"@en ;
    skos:scopeNote "Was previous \"Security\". Prefixed to distinguish from TechOrg measures."@en .

dpv-owl:EnterIntoContract a rdfs:Class,
        owl:Class,
        dpv-owl:LegalBasis ;
    dct:contributor "Georg P. Krog, Harshvardhan J. Pandit, Paul Ryan" ;
    dct:created "2021-04-07"^^xsd:date ;
    rdfs:isDefinedBy dpv-owl: ;
    rdfs:subClassOf dpv-owl:Contract ;
    sw:term_status "accepted"@en ;
    skos:definition "Processing necessary to enter into contract"@en ;
    skos:prefLabel "Enter Into Contract"@en .

dpv-owl:Entity a rdfs:Class,
        owl:Class ;
    dct:contributor "Harshvardhan J. Pandit" ;
    dct:created "2022-02-02"^^xsd:date ;
    rdfs:isDefinedBy dpv-owl: ;
    sw:term_status "accepted"@en ;
    skos:definition "A human or non-human 'thing' that constitutes as an entity"@en ;
    skos:prefLabel "Entity"@en .

dpv-owl:EntityActiveInvolvement a rdfs:Class,
        owl:Class ;
    dct:contributor "Delaram Golpayegani" ;
    dct:created "2024-05-11"^^xsd:date ;
    rdfs:isDefinedBy dpv-owl: ;
    rdfs:subClassOf dpv-owl:EntityInvolvement ;
    sw:term_status "accepted"@en ;
    skos:definition "Involvement where entity is 'actively' involved"@en ;
    skos:prefLabel "Entity Active Involvement"@en .

dpv-owl:EntityInformed a rdfs:Class,
        owl:Class,
        dpv-owl:EntityInformedStatus ;
    dct:contributor "Harshvardhan J. Pandit, Delaram Golpayegani, Georg P. Krog, Paul Ryan" ;
    dct:created "2024-05-10"^^xsd:date ;
    rdfs:isDefinedBy dpv-owl: ;
    rdfs:subClassOf dpv-owl:EntityInformedStatus ;
    sw:term_status "accepted"@en ;
    skos:definition "Status indicating entity has been informed about specified context"@en ;
    skos:prefLabel "Entity Informed"@en .

dpv-owl:EntityInformedStatus a rdfs:Class,
        owl:Class ;
    dct:contributor "Harshvardhan J. Pandit, Delaram Golpayegani, Georg P. Krog, Paul Ryan" ;
    dct:created "2024-05-10"^^xsd:date ;
    rdfs:isDefinedBy dpv-owl: ;
    rdfs:subClassOf dpv-owl:Status ;
    sw:term_status "accepted"@en ;
    skos:definition "Status indicating whether an entity is informed or uninformed about specified context"@en ;
    skos:prefLabel "Entity Informed Status"@en .

dpv-owl:EntityInvolvement a rdfs:Class,
        owl:Class ;
    dct:contributor "Harshvardhan J. Pandit, Delaram Golpayegani" ;
    dct:created "2024-05-11"^^xsd:date ;
    rdfs:isDefinedBy dpv-owl: ;
    rdfs:subClassOf dpv-owl:ProcessingContext ;
    sw:term_status "accepted"@en ;
    skos:definition "Involvement of an entity in specific context"@en ;
    skos:prefLabel "Entity Involvement"@en .

dpv-owl:EntityNonInvolvement a rdfs:Class,
        owl:Class ;
    dct:contributor "Delaram Golpayegani" ;
    dct:created "2024-05-11"^^xsd:date ;
    rdfs:isDefinedBy dpv-owl: ;
    rdfs:subClassOf dpv-owl:EntityInvolvement ;
    sw:term_status "accepted"@en ;
    skos:definition "Indicating entity is not involved"@en ;
    skos:prefLabel "Entity Non-Involvement"@en .

dpv-owl:EntityNonPermissiveInvolvement a rdfs:Class,
        owl:Class ;
    dct:contributor "Harshvardhan J. Pandit, Delaram Golpayegani" ;
    dct:created "2024-05-11"^^xsd:date ;
    rdfs:isDefinedBy dpv-owl: ;
    rdfs:subClassOf dpv-owl:EntityInvolvement ;
    sw:term_status "accepted"@en ;
    skos:definition "Involvement of an entity in specific context where it is not permitted or able to do something"@en ;
    skos:prefLabel "Entity Non-Permissive Involvement"@en .

dpv-owl:EntityPassiveInvolvement a rdfs:Class,
        owl:Class ;
    dct:contributor "Delaram Golpayegani" ;
    dct:created "2024-05-11"^^xsd:date ;
    rdfs:isDefinedBy dpv-owl: ;
    rdfs:subClassOf dpv-owl:EntityInvolvement ;
    sw:term_status "accepted"@en ;
    skos:definition "Involvement where entity is 'passively' or 'not actively' involved"@en ;
    skos:prefLabel "Entity Passive Involvement"@en .

dpv-owl:EntityPermissiveInvolvement a rdfs:Class,
        owl:Class ;
    dct:contributor "Harshvardhan J. Pandit, Delaram Golpayegani" ;
    dct:created "2024-05-11"^^xsd:date ;
    rdfs:isDefinedBy dpv-owl: ;
    rdfs:subClassOf dpv-owl:EntityInvolvement ;
    sw:term_status "accepted"@en ;
    skos:definition "Involvement of an entity in specific context where it is permitted or able to do something"@en ;
    skos:prefLabel "Entity Permissive Involvement"@en .

dpv-owl:EntityUninformed a rdfs:Class,
        owl:Class ;
    dct:contributor "Harshvardhan J. Pandit, Delaram Golpayegani, Georg P. Krog, Paul Ryan" ;
    dct:created "2024-05-10"^^xsd:date ;
    rdfs:isDefinedBy dpv-owl: ;
    rdfs:subClassOf dpv-owl:EntityInformedStatus ;
    sw:term_status "accepted"@en ;
    skos:definition "Status indicating entity is uninformed i.e. has been not been informed about specified context"@en ;
    skos:prefLabel "Entity Uninformed"@en .

dpv-owl:EnvironmentalProtection a rdfs:Class,
        owl:Class,
        dpv-owl:PhysicalMeasure ;
    dct:contributor "Harshvardhan J. Pandit" ;
    dct:created "2024-04-14"^^xsd:date ;
    dct:source "NIST SP 800-13"@en ;
    rdfs:isDefinedBy dpv-owl: ;
    rdfs:subClassOf dpv-owl:PhysicalMeasure ;
    sw:term_status "accepted"@en ;
    skos:definition "Physical protection against environmental threats such as fire, floods, storms, etc."@en ;
    skos:prefLabel "Environmental Protection"@en .

dpv-owl:Erase a rdfs:Class,
        owl:Class,
        dpv-owl:Processing ;
    dct:created "2019-05-07"^^xsd:date ;
    dct:source [ a schema:WebPage ;
            schema:name "GDPR Art.4-2" ;
            schema:url "https://eur-lex.europa.eu/eli/reg/2016/679/art_4/par_2/oj" ] ;
    rdfs:isDefinedBy dpv-owl: ;
    rdfs:subClassOf dpv-owl:Remove ;
    sw:term_status "accepted"@en ;
    skos:definition "to remove data from existence i.e. without the possibility of retrieval"@en ;
    skos:prefLabel "Erase"@en .

dpv-owl:EstablishContractualAgreement a rdfs:Class,
        owl:Class,
        dpv-owl:Purpose ;
    dct:contributor "Georg P. Krog, Harshvardhan J. Pandit" ;
    dct:created "2022-11-09"^^xsd:date ;
    rdfs:isDefinedBy dpv-owl: ;
    rdfs:subClassOf dpv-owl:Purpose ;
    sw:term_status "accepted"@en ;
    skos:definition "Purposes associated with carrying out data processing to establish an agreement, such as for entering into a contract"@en ;
    skos:prefLabel "Establish Contractual Agreement"@en .

dpv-owl:EvaluationOfIndividuals a rdfs:Class,
        owl:Class,
        dpv-owl:EvaluationScoring ;
    dct:contributor "Harshvardhan J. Pandit" ;
    dct:created "2022-10-22"^^xsd:date ;
    dct:modified "2022-11-30"^^xsd:date ;
    dct:source [ a schema:WebPage ;
            schema:name "GDPR Art.4-2" ;
            schema:url "https://eur-lex.europa.eu/eli/reg/2016/679/art_4/par_2/oj" ] ;
    rdfs:isDefinedBy dpv-owl: ;
    rdfs:subClassOf dpv-owl:EvaluationScoring ;
    sw:term_status "accepted"@en ;
    skos:definition "Processing that involves evaluation of individuals"@en ;
    skos:prefLabel "Evaluation of Individuals"@en .

dpv-owl:EvaluationScoring a rdfs:Class,
        owl:Class ;
    dct:contributor "Harshvardhan J. Pandit, Piero Bonatti" ;
    dct:created "2020-11-04"^^xsd:date ;
    dct:source [ a schema:WebPage ;
            schema:name "GDPR Art.4-2" ;
            schema:url "https://eur-lex.europa.eu/eli/reg/2016/679/art_4/par_2/oj" ] ;
    rdfs:isDefinedBy dpv-owl: ;
    rdfs:subClassOf dpv-owl:ProcessingContext ;
    sw:term_status "accepted"@en ;
    skos:definition "Processing that involves evaluation and scoring of individuals"@en ;
    skos:prefLabel "Evaluation and Scoring"@en .

dpv-owl:ExpectationStatus a rdfs:Class,
        owl:Class ;
    dct:contributor "Harshvardhan J. Pandit, Delaram Golpayegani, Georg P. Krog, Paul Ryan" ;
    dct:created "2024-05-10"^^xsd:date ;
    rdfs:isDefinedBy dpv-owl: ;
    sw:term_status "accepted"@en ;
    skos:definition "Status indicating whether the specified context was intended or unintended"@en ;
    skos:prefLabel "Expectation Status"@en ;
    skos:scopeNote "Expectation is associated with the outcome of a goal or purpose for what is expected to happen i.e. an ex-post indication of what was expected to happen in the specified context. Intention and Expectation are closely related terms. We recommend using Intention when the entity has the ability to control the implementation and Expectation for when the entity does not have control or for what happens after or beyond the exercise of control."@en .

dpv-owl:Expected a rdfs:Class,
        owl:Class,
        dpv-owl:ExpectationStatus ;
    dct:contributor "Harshvardhan J. Pandit, Delaram Golpayegani, Georg P. Krog, Paul Ryan" ;
    dct:created "2024-05-10"^^xsd:date ;
    rdfs:isDefinedBy dpv-owl: ;
    rdfs:subClassOf dpv-owl:ExpectationStatus ;
    sw:term_status "accepted"@en ;
    skos:definition "Status indicating the specified context was expected"@en ;
    skos:prefLabel "Expected"@en .

dpv-owl:ExplicitlyExpressedConsent a rdfs:Class,
        owl:Class,
        dpv-owl:LegalBasis ;
    dct:contributor "Georg P. Krog, Harshvardhan J. Pandit, Paul Ryan, Julian Flake" ;
    dct:created "2022-06-21"^^xsd:date ;
    vann:example dex-owl:E0018 ;
    rdfs:isDefinedBy dpv-owl: ;
    rdfs:subClassOf dpv-owl:ExpressedConsent ;
    sw:term_status "accepted"@en ;
    skos:definition "Consent that is expressed through an explicit action solely conveying a consenting decision"@en ;
    skos:prefLabel "Explicitly Expressed Consent"@en ;
    skos:scopeNote "Explicitly expressed consent is a more specific form of Expressed consent where the action taken must 'explicitly' relate to only the consent decision. Expressed consent where the consenting is part of other matters therefore cannot satisfy the requirements of explicitly expressed consent. An example of explicit action expressing the consenting decision is a button on a web form where the form only relates to consent, or it is accompanied with suitable text that reiterates what the consenting decision is about"@en .

dpv-owl:Export a rdfs:Class,
        owl:Class,
        dpv-owl:Processing ;
    dct:contributor "Beatriz Esteves" ;
    dct:created "2024-04-14"^^xsd:date ;
    dct:source "DGA 2.20"@en ;
    rdfs:isDefinedBy dpv-owl: ;
    rdfs:subClassOf dpv-owl:Disclose ;
    sw:term_status "accepted"@en ;
    skos:definition "to provide a copy of data from one system to another"@en ;
    skos:prefLabel "Export"@en .

dpv-owl:ExpressedConsent a rdfs:Class,
        owl:Class,
        dpv-owl:LegalBasis ;
    dct:contributor "Georg P. Krog, Harshvardhan J. Pandit, Paul Ryan, Julian Flake" ;
    dct:created "2022-06-21"^^xsd:date ;
    vann:example dex-owl:E0018 ;
    rdfs:isDefinedBy dpv-owl: ;
    rdfs:subClassOf dpv-owl:InformedConsent ;
    sw:term_status "accepted"@en ;
    skos:definition "Consent that is expressed through an action intended to convey a consenting decision"@en ;
    skos:prefLabel "Expressed Consent"@en ;
    skos:scopeNote "Expressed consent requires the individual take a specific and unambiguous action that directly indicates their consent. This action may be a part of other processes such as setting preferences, or agreeing to a contract, or other matters not relating to consent. An example of expressed consent is interacting with a checkbox within a dashboard or clicking a button on a web form"@en .

dpv-owl:FRIA a rdfs:Class,
        owl:Class,
        dpv-owl:OrganisationalMeasure ;
    dct:contributor "Harshvardhan J. Pandit" ;
    dct:created "2024-04-14"^^xsd:date ;
    dct:source "AI Act Art.27"@en ;
    rdfs:isDefinedBy dpv-owl: ;
    rdfs:subClassOf dpv-owl:RightsImpactAssessment ;
    sw:term_status "accepted"@en ;
    skos:definition "Impact assessment which assesses the potential and actual impact on fundamental rights occuring due to processing activities"@en ;
    skos:prefLabel "Fundamental Rights Impact Assessment (FRIA)"@en ;
    skos:scopeNote "The fundamental rights and freedoms may be those defined in law or other norms, and may be bound to a jurisdiction - for example see EU Charter of Fundamental Rights"@en .

dpv-owl:FederatedLocations a rdfs:Class,
        owl:Class,
        dpv-owl:LocationFixture ;
    dct:contributor "Harshvardhan J. Pandit" ;
    dct:created "2022-06-15"^^xsd:date ;
    dct:modified "2020-10-05"^^xsd:date ;
    rdfs:isDefinedBy dpv-owl: ;
    rdfs:subClassOf dpv-owl:LocationFixture ;
    sw:term_status "accepted"@en ;
    skos:definition "Location that is federated across multiple separate areas with designation of a primary or central location"@en ;
    skos:prefLabel "Federated Locations"@en .

dpv-owl:FileSystemSecurity a rdfs:Class,
        owl:Class,
        dpv-owl:TechnicalMeasure ;
    dct:contributor "Harshvardhan J. Pandit" ;
    dct:created "2022-08-17"^^xsd:date ;
    dct:source [ a schema:WebPage ;
            schema:name "ENISA Reference Incident Classification Taxonomy 2018" ;
            schema:url "https://www.enisa.europa.eu/publications/reference-incident-classification-taxonomy/" ] ;
    rdfs:isDefinedBy dpv-owl: ;
    rdfs:subClassOf dpv-owl:SecurityMethod ;
    sw:term_status "accepted"@en ;
    skos:definition "Security implemented over a file system"@en ;
    skos:prefLabel "File System Security"@en .

dpv-owl:Filter a rdfs:Class,
        owl:Class,
        dpv-owl:Processing ;
    dct:contributor "Harshvardhan J. Pandit, Georg P. Krog" ;
    dct:created "2022-06-15"^^xsd:date ;
    rdfs:isDefinedBy dpv-owl: ;
    rdfs:subClassOf dpv-owl:Transform ;
    sw:term_status "accepted"@en ;
    skos:definition "to filter or keep data for some criteria"@en ;
    skos:prefLabel "Filter"@en .

dpv-owl:FixedLocation a rdfs:Class,
        owl:Class,
        dpv-owl:LocationFixture ;
    dct:contributor "Harshvardhan J. Pandit" ;
    dct:created "2022-06-15"^^xsd:date ;
    dct:modified "2020-10-05"^^xsd:date ;
    rdfs:isDefinedBy dpv-owl: ;
    rdfs:subClassOf dpv-owl:LocationFixture ;
    sw:term_status "accepted"@en ;
    skos:definition "Location that is fixed i.e. known to occur at a specific place"@en ;
    skos:prefLabel "Fixed Location"@en .

dpv-owl:FixedMultipleLocations a rdfs:Class,
        owl:Class,
        dpv-owl:LocationFixture ;
    dct:contributor "Harshvardhan J. Pandit" ;
    dct:created "2022-06-15"^^xsd:date ;
    dct:modified "2020-10-05"^^xsd:date ;
    rdfs:isDefinedBy dpv-owl: ;
    rdfs:subClassOf dpv-owl:FixedLocation ;
    sw:term_status "accepted"@en ;
    skos:definition "Location that is fixed with multiple places e.g. multiple cities"@en ;
    skos:prefLabel "Fixed Multiple Locations"@en .

dpv-owl:FixedOccurrencesDuration a rdfs:Class,
        owl:Class ;
    dct:contributor "Harshvardhan J. Pandit" ;
    dct:created "2022-06-15"^^xsd:date ;
    dct:modified "2020-10-05"^^xsd:date ;
    rdfs:isDefinedBy dpv-owl: ;
    rdfs:subClassOf dpv-owl:Duration ;
    sw:term_status "accepted"@en ;
    skos:definition "Duration that takes place a fixed number of times e.g. 3 times"@en ;
    skos:prefLabel "Fixed Occurrences Duration"@en .

dpv-owl:FixedSingularLocation a rdfs:Class,
        owl:Class,
        dpv-owl:LocationFixture ;
    dct:contributor "Harshvardhan J. Pandit" ;
    dct:created "2022-06-15"^^xsd:date ;
    dct:modified "2020-10-05"^^xsd:date ;
    rdfs:isDefinedBy dpv-owl: ;
    rdfs:subClassOf dpv-owl:FixedLocation ;
    sw:term_status "accepted"@en ;
    skos:definition "Location that is fixed at a specific place e.g. a city"@en ;
    skos:prefLabel "Fixed Singular Location"@en .

dpv-owl:ForProfitOrganisation a rdfs:Class,
        owl:Class ;
    dct:contributor "Harshvardhan J. Pandit" ;
    dct:created "2022-02-02"^^xsd:date ;
    dct:modified "2020-10-05"^^xsd:date ;
    rdfs:isDefinedBy dpv-owl: ;
    rdfs:subClassOf dpv-owl:Organisation ;
    sw:term_status "accepted"@en ;
    skos:definition "An organisation that aims to achieve profit as its primary goal"@en ;
    skos:prefLabel "For-Profit Organisation"@en .

dpv-owl:Format a rdfs:Class,
        owl:Class,
        dpv-owl:Processing ;
    dct:contributor "Beatriz Esteves" ;
    dct:created "2024-04-14"^^xsd:date ;
    dct:source "DGA 12.d"@en ;
    rdfs:isDefinedBy dpv-owl: ;
    rdfs:subClassOf dpv-owl:Structure ;
    sw:term_status "accepted"@en ;
    skos:definition "to arrange or structure data in a specific form"@en ;
    skos:prefLabel "Format"@en .

dpv-owl:FraudPreventionAndDetection a rdfs:Class,
        owl:Class,
        dpv-owl:Purpose ;
    dct:contributor "Harshvardhan J. Pandit, Javier Fernández, Axel Polleres, Elmar Kiesling, Fajar Ekaputra, Simon Steyskal" ;
    dct:created "2019-04-05"^^xsd:date ;
    rdfs:isDefinedBy dpv-owl: ;
    rdfs:subClassOf dpv-owl:MisusePreventionAndDetection ;
    sw:term_status "accepted"@en ;
    skos:definition "Purposes associated with fraud detection, prevention, and mitigation"@en ;
    skos:prefLabel "Fraud Prevention and Detection"@en ;
    skos:related svpu:Government .

dpv-owl:Frequency a rdfs:Class,
        owl:Class ;
    dct:contributor "Harshvardhan J. Pandit" ;
    dct:created "2022-02-16"^^xsd:date ;
    vann:example dex-owl:E0051 ;
    rdfs:isDefinedBy dpv-owl: ;
    rdfs:subClassOf dpv-owl:Context ;
    sw:term_status "accepted"@en ;
    skos:definition "The frequency or information about periods and repetitions in terms of recurrence."@en ;
    skos:prefLabel "Frequency"@en .

dpv-owl:FulfilmentOfContractualObligation a rdfs:Class,
        owl:Class,
        dpv-owl:Purpose ;
    dct:contributor "Georg P. Krog, Harshvardhan J. Pandit" ;
    dct:created "2022-11-09"^^xsd:date ;
    rdfs:isDefinedBy dpv-owl: ;
    rdfs:subClassOf dpv-owl:FulfilmentOfObligation ;
    sw:term_status "accepted"@en ;
    skos:definition "Purposes associated with carrying out data processing to fulfill a contractual obligation"@en ;
    skos:prefLabel "Fulfilment of Contractual Obligation"@en .

dpv-owl:FulfilmentOfObligation a rdfs:Class,
        owl:Class,
        dpv-owl:Purpose ;
    dct:contributor "Georg P. Krog, Harshvardhan J. Pandit" ;
    dct:created "2022-11-09"^^xsd:date ;
    rdfs:isDefinedBy dpv-owl: ;
    rdfs:subClassOf dpv-owl:Purpose ;
    sw:term_status "accepted"@en ;
    skos:definition "Purposes associated with carrying out data processing to fulfill an obligation"@en ;
    skos:prefLabel "Fulfilment of Obligation"@en .

dpv-owl:FullAutomation a rdfs:Class,
        owl:Class,
        dpv-owl:AutomationLevel ;
    dct:contributor "Harshvardhan J. Pandit, Delaram Golpayegani" ;
    dct:created "2023-12-10"^^xsd:date ;
    dct:modified "2024-04-20"^^xsd:date ;
    dct:source [ a schema:WebPage ;
            schema:name "ISO/IEC 22989:2022 Artificial intelligence concepts and terminology" ;
            schema:url "https://www.iso.org/standard/74296.html" ] ;
    rdfs:isDefinedBy dpv-owl: ;
    rdfs:subClassOf dpv-owl:AutomationLevel ;
    sw:term_status "accepted"@en ;
    skos:definition "Level of automation corresponding to Level 5 in ISO/IEC 22989:2022 where the automation in system is capable of performing all its tasks regardless of the conditions without human involvement"@en ;
    skos:prefLabel "Full Automation"@en ;
    skos:scopeNote "Though Fully Automated such operations can still be associated with dpv:HumanInvolved e.g. for inputs, oversight or verification"@en .

dpv-owl:FullyRandomisedPseudonymisation a rdfs:Class,
        owl:Class,
        dpv-owl:TechnicalMeasure ;
    dct:contributor "Harshvardhan J. Pandit" ;
    dct:created "2022-08-17"^^xsd:date ;
    dct:source [ a schema:WebPage ;
            schema:name "ENISA Data Pseudonymisation: Advanced Techniques and Use Cases" ;
            schema:url "https://www.enisa.europa.eu/publications/data-pseudonymisation-advanced-techniques-and-use-cases" ] ;
    rdfs:isDefinedBy dpv-owl: ;
    rdfs:subClassOf dpv-owl:Pseudonymisation ;
    sw:term_status "accepted"@en ;
    skos:definition "Use of randomised pseudonymisation where the same elements are assigned different values each time they occur"@en ;
    skos:prefLabel "Fully Randomised Pseudonymisation"@en .

dpv-owl:Generate a rdfs:Class,
        owl:Class,
        dpv-owl:Processing ;
    dct:contributor "Harshvardhan J. Pandit" ;
    dct:created "2022-04-20"^^xsd:date ;
    rdfs:isDefinedBy dpv-owl: ;
    rdfs:subClassOf dpv-owl:Obtain ;
    sw:term_status "accepted"@en ;
    skos:definition "to generate or create data"@en ;
    skos:prefLabel "Generate"@en .

dpv-owl:GeneratedData a rdfs:Class,
        owl:Class ;
    dct:created "2023-12-10"^^xsd:date ;
    rdfs:isDefinedBy dpv-owl: ;
    rdfs:subClassOf dpv-owl:Data ;
    sw:term_status "accepted"@en ;
    skos:definition "Data that is generated or brought into existence without relation to existing data i.e. it is not derived or inferred from other data"@en ;
    skos:prefLabel "Generated Data"@en .

dpv-owl:GeneratedPersonalData a rdfs:Class,
        owl:Class ;
    dct:contributor "Harshvardhan J. Pandit" ;
    dct:created "2022-03-30"^^xsd:date ;
    dct:modified "2023-12-10"^^xsd:date ;
    rdfs:isDefinedBy dpv-owl: ;
    rdfs:subClassOf dpv-owl:PersonalData ;
    sw:term_status "accepted"@en ;
    skos:definition "Personal Data that is generated or brought into existence without relation to existing data i.e. it is not derived or inferred from other data"@en ;
    skos:prefLabel "Generated Personal Data"@en ;
    skos:scopeNote "Generated Data is used to indicate data that is produced and is not derived or inferred from other data"@en .

dpv-owl:GeographicCoverage a rdfs:Class,
        owl:Class ;
    dct:contributor "Harshvardhan J. Pandit, Georg P. Krog, Paul Ryan" ;
    dct:created "2022-06-15"^^xsd:date ;
    vann:example dex-owl:E0049 ;
    rdfs:isDefinedBy dpv-owl: ;
    rdfs:subClassOf dpv-owl:Scale ;
    sw:term_status "accepted"@en ;
    skos:definition "Indicate of scale in terms of geographic coverage"@en ;
    skos:prefLabel "Geographic Coverage"@en .

dpv-owl:GlobalScale a rdfs:Class,
        owl:Class,
        dpv-owl:GeographicCoverage ;
    dct:contributor "Harshvardhan J. Pandit" ;
    dct:created "2022-06-15"^^xsd:date ;
    rdfs:isDefinedBy dpv-owl: ;
    rdfs:subClassOf dpv-owl:GeographicCoverage ;
    sw:term_status "accepted"@en ;
    skos:definition "Geographic coverage spanning the entire globe"@en ;
    skos:prefLabel "Global Scale"@en .

dpv-owl:GovernanceProcedures a rdfs:Class,
        owl:Class,
        dpv-owl:OrganisationalMeasure ;
    dct:contributor "Harshvardhan J. Pandit" ;
    dct:created "2022-08-17"^^xsd:date ;
    dct:source [ a schema:WebPage ;
            schema:name "ENISA 5G Cybersecurity Standards" ;
            schema:url "https://www.enisa.europa.eu/publications/5g-cybersecurity-standards" ] ;
    rdfs:isDefinedBy dpv-owl: ;
    rdfs:subClassOf dpv-owl:OrganisationalMeasure ;
    sw:term_status "accepted"@en ;
    skos:definition "Procedures related to governance (e.g. organisation, unit, team, process, system)"@en ;
    skos:prefLabel "Governance Procedures"@en .

dpv-owl:GovernmentalOrganisation a rdfs:Class,
        owl:Class ;
    dct:contributor "Harshvardhan J. Pandit" ;
    dct:created "2022-02-02"^^xsd:date ;
    dct:modified "2020-10-05"^^xsd:date ;
    rdfs:isDefinedBy dpv-owl: ;
    rdfs:subClassOf dpv-owl:Organisation ;
    sw:term_status "accepted"@en ;
    skos:definition "An organisation managed or part of government"@en ;
    skos:prefLabel "Governmental Organisation"@en .

dpv-owl:GuardianOfDataSubject a rdfs:Class,
        owl:Class,
        dpv-owl:DataSubject ;
    dct:contributor "Georg P. Krog" ;
    dct:created "2022-08-03"^^xsd:date ;
    rdfs:isDefinedBy dpv-owl: ;
    rdfs:subClassOf dpv-owl:DataSubject ;
    sw:term_status "accepted"@en ;
    skos:definition "Guardian(s) of data subjects such as children"@en ;
    skos:prefLabel "Guardian(s) of Data Subject"@en .

dpv-owl:Guideline a rdfs:Class,
        owl:Class,
        dpv-owl:OrganisationalMeasure ;
    dct:contributor "Harshvardhan J. Pandit" ;
    dct:created "2024-05-12"^^xsd:date ;
    rdfs:isDefinedBy dpv-owl: ;
    rdfs:subClassOf dpv-owl:GuidelinesPrinciple ;
    sw:term_status "accepted"@en ;
    skos:definition "Practices that specify how activities must be conducted"@en ;
    skos:prefLabel "Guideline"@en .

dpv-owl:GuidelinesPrinciple a rdfs:Class,
        owl:Class,
        dpv-owl:OrganisationalMeasure ;
    dct:contributor "Axel Polleres, Rob Brennan, Harshvardhan J. Pandit, Mark Lizar" ;
    dct:created "2019-04-05"^^xsd:date ;
    rdfs:isDefinedBy dpv-owl: ;
    rdfs:subClassOf dpv-owl:OrganisationalMeasure ;
    sw:term_status "accepted"@en ;
    skos:definition "Guidelines or Principles regarding processing and operational measures"@en ;
    skos:prefLabel "Guidelines Principle"@en .

dpv-owl:HardwareSecurityProtocols a rdfs:Class,
        owl:Class,
        dpv-owl:TechnicalMeasure ;
    dct:contributor "Harshvardhan J. Pandit" ;
    dct:created "2022-08-17"^^xsd:date ;
    dct:source [ a schema:WebPage ;
            schema:name "ENISA Reference Incident Classification Taxonomy 2018" ;
            schema:url "https://www.enisa.europa.eu/publications/reference-incident-classification-taxonomy/" ] ;
    rdfs:isDefinedBy dpv-owl: ;
    rdfs:subClassOf dpv-owl:SecurityMethod ;
    sw:term_status "accepted"@en ;
    skos:definition "Security protocols implemented at or within hardware"@en ;
    skos:prefLabel "Hardware Security Protocols"@en .

dpv-owl:HashFunctions a rdfs:Class,
        owl:Class,
        dpv-owl:TechnicalMeasure ;
    dct:contributor "Harshvardhan J. Pandit" ;
    dct:created "2022-08-17"^^xsd:date ;
    dct:source [ a schema:WebPage ;
            schema:name "ENISA Reference Incident Classification Taxonomy 2018" ;
            schema:url "https://www.enisa.europa.eu/publications/reference-incident-classification-taxonomy/" ] ;
    rdfs:isDefinedBy dpv-owl: ;
    rdfs:subClassOf dpv-owl:CryptographicMethods ;
    sw:term_status "accepted"@en ;
    skos:definition "Use of hash functions to map information or to retrieve a prior categorisation"@en ;
    skos:prefLabel "Hash Functions"@en .

dpv-owl:HashMessageAuthenticationCode a rdfs:Class,
        owl:Class,
        dpv-owl:TechnicalMeasure ;
    dct:contributor "Harshvardhan J. Pandit" ;
    dct:created "2022-08-17"^^xsd:date ;
    dct:source [ a schema:WebPage ;
            schema:name "ENISA 5G Cybersecurity Standards" ;
            schema:url "https://www.enisa.europa.eu/publications/5g-cybersecurity-standards" ] ;
    rdfs:isDefinedBy dpv-owl: ;
    rdfs:subClassOf dpv-owl:CryptographicAuthentication ;
    sw:term_status "accepted"@en ;
    skos:definition "Use of HMAC where message authentication code (MAC) utilise a cryptographic hash function and a secret cryptographic key"@en ;
    skos:prefLabel "Hash-based Message Authentication Code (HMAC)"@en .

dpv-owl:HighAutomation a rdfs:Class,
        owl:Class,
        dpv-owl:AutomationLevel ;
    dct:contributor "Harshvardhan J. Pandit, Delaram Golpayegani" ;
    dct:created "2023-12-10"^^xsd:date ;
    dct:modified "2024-04-20"^^xsd:date ;
    dct:source [ a schema:WebPage ;
            schema:name "ISO/IEC 22989:2022 Artificial intelligence concepts and terminology" ;
            schema:url "https://www.iso.org/standard/74296.html" ] ;
    rdfs:isDefinedBy dpv-owl: ;
    rdfs:subClassOf dpv-owl:AutomationLevel ;
    sw:term_status "accepted"@en ;
    skos:definition "Level of automation corresponding to Level 4 in ISO/IEC 22989:2022 where the automation in system is capable of performing all its tasks within specific controlled conditions without human involvement"@en ;
    skos:prefLabel "High Automation"@en ;
    skos:scopeNote "Human Involvement is implied here, e.g. for intervention, input, decisions"@en .

dpv-owl:HomomorphicEncryption a rdfs:Class,
        owl:Class,
        dpv-owl:TechnicalMeasure ;
    dct:contributor "Harshvardhan J. Pandit" ;
    dct:created "2022-08-17"^^xsd:date ;
    dct:source [ a schema:WebPage ;
            schema:name "ENISA Reference Incident Classification Taxonomy 2018" ;
            schema:url "https://www.enisa.europa.eu/publications/reference-incident-classification-taxonomy/" ] ;
    rdfs:isDefinedBy dpv-owl: ;
    rdfs:subClassOf dpv-owl:CryptographicMethods ;
    sw:term_status "accepted"@en ;
    skos:definition "Use of Homomorphic encryption that permits computations on encrypted data without decrypting it"@en ;
    skos:prefLabel "Homomorphic Encryption"@en .

dpv-owl:HugeDataVolume a rdfs:Class,
        owl:Class,
        dpv-owl:DataVolume ;
    dct:contributor "Harshvardhan J. Pandit" ;
    dct:created "2022-06-15"^^xsd:date ;
    rdfs:isDefinedBy dpv-owl: ;
    rdfs:subClassOf dpv-owl:DataVolume ;
    sw:term_status "accepted"@en ;
    skos:definition "Data volume that is considered huge or more than large within the context"@en ;
    skos:prefLabel "Huge Data Volume"@en .

dpv-owl:HugeScaleOfDataSubjects a rdfs:Class,
        owl:Class,
        dpv-owl:DataSubjectScale ;
    dct:contributor "Harshvardhan J. Pandit" ;
    dct:created "2022-06-15"^^xsd:date ;
    rdfs:isDefinedBy dpv-owl: ;
    rdfs:subClassOf dpv-owl:DataSubjectScale ;
    sw:term_status "accepted"@en ;
    skos:definition "Scale of data subjects considered huge or more than large within the context"@en ;
    skos:prefLabel "Huge Scale Of Data Subjects"@en .

dpv-owl:HumanInvolved a rdfs:Class,
        owl:Class,
        dpv-owl:HumanInvolvement ;
    dct:created "2022-09-03"^^xsd:date ;
    dct:modified "2023-12-10"^^xsd:date ;
    rdfs:isDefinedBy dpv-owl: ;
    rdfs:subClassOf dpv-owl:HumanInvolvement ;
    sw:term_status "accepted"@en ;
    skos:definition "Humans are involved in the specified context"@en ;
    skos:prefLabel "Human involved"@en ;
    skos:scopeNote "This concept only indicates that humans are involved. For specific involvement, see specialised concepts e.g. involved for input, oversight."@en .

dpv-owl:HumanInvolvement a rdfs:Class,
        owl:Class ;
    dct:contributor "Harshvardhan J. Pandit" ;
    dct:created "2022-01-26"^^xsd:date ;
    dct:modified "2024-04-20"^^xsd:date ;
    vann:example dex-owl:E0013 ;
    rdfs:isDefinedBy dpv-owl: ;
    rdfs:subClassOf dpv-owl:EntityInvolvement ;
    sw:term_status "accepted"@en ;
    skos:definition "The involvement of humans in specified context"@en ;
    skos:prefLabel "Human Involvement"@en ;
    skos:scopeNote "Human Involvement here broadly refers to any involvement by a human in the context of carrying out processing. This may include verification of outcomes, providing input data for making decisions, or overseeing activities. To indicate whether humans are involved or not, see relevant concepts of dpv:HumanInvolved and dpv:HumanNotInvolved. The term 'Human in the loop' and its varieties are absent from DPV due to their contradictory and non-compatible use across different sources."@en .

dpv-owl:HumanInvolvementForControl a rdfs:Class,
        owl:Class,
        dpv-owl:HumanInvolvement ;
    dct:created "2022-09-04"^^xsd:date ;
    dct:modified "2023-12-10"^^xsd:date ;
    rdfs:isDefinedBy dpv-owl: ;
    rdfs:subClassOf dpv-owl:HumanInvolvement ;
    sw:term_status "accepted"@en ;
    skos:definition "Human involvement for the purposes of exercising control over the specified operations in context"@en ;
    skos:prefLabel "Human Involvement for control"@en ;
    skos:scopeNote "Control is a broad term that can be applied to various stages and operations. It maps to None, Assistive, and Partial automation models."@en .

dpv-owl:HumanInvolvementForDecision a rdfs:Class,
        owl:Class,
        dpv-owl:HumanInvolvement ;
    dct:created "2022-09-06"^^xsd:date ;
    dct:modified "2023-12-10"^^xsd:date ;
    rdfs:isDefinedBy dpv-owl: ;
    rdfs:subClassOf dpv-owl:HumanInvolvement ;
    sw:term_status "accepted"@en ;
    skos:definition "Human involvement for the purposes of exercising decisions over the specified operations in context"@en ;
    skos:prefLabel "Human Involvement for decision"@en ;
    skos:scopeNote "Decisions are about exercising control over the operation, and are distinct from input (data or parameters)."@en .

dpv-owl:HumanInvolvementForInput a rdfs:Class,
        owl:Class,
        dpv-owl:HumanInvolvement ;
    dct:contributor "Harshvardhan J. Pandit" ;
    dct:created "2022-09-07"^^xsd:date ;
    dct:modified "2023-12-10"^^xsd:date ;
    rdfs:isDefinedBy dpv-owl: ;
    rdfs:subClassOf dpv-owl:HumanInvolvement ;
    sw:term_status "accepted"@en ;
    skos:definition "Human involvement for the purposes of providing inputs to the specified context"@en ;
    skos:prefLabel "Human Involvement for Input"@en ;
    skos:scopeNote "Inputs can be in the form of data or other resources."@en .

dpv-owl:HumanInvolvementForIntervention a rdfs:Class,
        owl:Class,
        dpv-owl:HumanInvolvement ;
    dct:created "2022-09-05"^^xsd:date ;
    dct:modified "2023-12-10"^^xsd:date ;
    rdfs:isDefinedBy dpv-owl: ;
    rdfs:subClassOf dpv-owl:HumanInvolvement ;
    sw:term_status "accepted"@en ;
    skos:definition "Human involvement for the purposes of exercising interventions over the specified operations in context"@en ;
    skos:prefLabel "Human Involvement for intervention"@en ;
    skos:scopeNote "Intervention indicates the ability to intervene in operations, which can be at various stages. It maps to Conditional and High automation models."@en .

dpv-owl:HumanInvolvementForOversight a rdfs:Class,
        owl:Class,
        dpv-owl:HumanInvolvement ;
    dct:contributor "Harshvardhan J. Pandit" ;
    dct:created "2022-09-07"^^xsd:date ;
    dct:modified "2023-12-10"^^xsd:date ;
    rdfs:isDefinedBy dpv-owl: ;
    rdfs:subClassOf dpv-owl:HumanInvolvement ;
    sw:term_status "accepted"@en ;
    skos:definition "Human involvement for the purposes of having oversight over the specified context regarding its operations, inputs, or outputs"@en ;
    skos:prefLabel "Human Involvement for Oversight"@en ;
    skos:scopeNote "Oversight by itself does not indicate the ability to intervene or control the operations."@en .

dpv-owl:HumanInvolvementForVerification a rdfs:Class,
        owl:Class,
        dpv-owl:HumanInvolvement ;
    dct:contributor "Harshvardhan J. Pandit" ;
    dct:created "2022-09-07"^^xsd:date ;
    dct:modified "2023-12-10"^^xsd:date ;
    rdfs:isDefinedBy dpv-owl: ;
    rdfs:subClassOf dpv-owl:HumanInvolvement ;
    sw:term_status "accepted"@en ;
    skos:definition "Human involvement for the purposes of verification of specified context to ensure its operations, inputs, or outputs are correct or are acceptable."@en ;
    skos:prefLabel "Human Involvement for Verification"@en ;
    skos:scopeNote "Verification by itself does not imply ability to Control, Intervene, or having Oversight."@en .

dpv-owl:HumanNotInvolved a rdfs:Class,
        owl:Class,
        dpv-owl:HumanInvolvement ;
    dct:created "2023-12-10"^^xsd:date ;
    rdfs:isDefinedBy dpv-owl: ;
    rdfs:subClassOf dpv-owl:HumanInvolvement ;
    sw:term_status "accepted"@en ;
    skos:definition "Humans are not involved in the specified context"@en ;
    skos:prefLabel "Human not involved"@en ;
    skos:scopeNote "This maps to Autonomous and Full Automation models if no humans are involved."@en .

dpv-owl:HumanResourceManagement a rdfs:Class,
        owl:Class,
        dpv-owl:Purpose ;
    dct:contributor "Paul Ryan, David Hickey, Georg P. Krog, Harshvardhan J. Pandit, Beatriz Esteves" ;
    dct:created "2021-09-01"^^xsd:date ;
    dct:source [ a schema:WebPage ;
            schema:name "Belgian DPA ROPA Template" ;
            schema:url "https://www.privacycommission.be/nl/model-voor-een-register-van-de-verwerkingsactiviteiten" ] ;
    rdfs:isDefinedBy dpv-owl: ;
    rdfs:subClassOf dpv-owl:Purpose ;
    sw:term_status "accepted"@en ;
    skos:definition "Purposes associated with managing humans and 'human resources' within the organisation for effective and efficient operations."@en ;
    skos:prefLabel "Human Resource Management"@en ;
    skos:scopeNote "HR is a broad concept. Its management includes, amongst others - recruiting employees and intermediaries e.g. brokers, independent representatives; payroll administration, remunerations, commissions, and wages; and application of social legislation."@en .

dpv-owl:IPRManagement a rdfs:Class,
        owl:Class,
        dpv-owl:OrganisationalMeasure ;
    dct:contributor "Beatriz Esteves, Harshvardhan J. Pandit, Georg P. Krog" ;
    dct:created "2024-04-14"^^xsd:date ;
    dct:source "DGA 3.1.c"@en ;
    rdfs:isDefinedBy dpv-owl: ;
    rdfs:subClassOf dpv-owl:RightsManagement ;
    sw:term_status "accepted"@en ;
    skos:definition "Management of Intellectual Property Rights with a view to identify and safeguard and enforce them"@en ;
    skos:prefLabel "Intellectual Property Rights Management"@en .

dpv-owl:IdentifyingPersonalData a rdfs:Class,
        owl:Class ;
    dct:created "2024-02-14"^^xsd:date ;
    rdfs:isDefinedBy dpv-owl: ;
    rdfs:subClassOf dpv-owl:PersonalData ;
    sw:term_status "accepted"@en ;
    skos:definition "Personal Data that explicitly and by itself is sufficient to identify a person"@en ;
    skos:prefLabel "Identifying Personal Data"@en ;
    skos:scopeNote "DPV does not use PII ('Personally Identifiable Information') as it has varying and conflicting definitions across sources. Instead the concept 'identifying personal data' is intended to provide a clear categorisation of its interpretation. Where multiple data categories can be combined to create an 'identifying' category e.g. fingerprinting, this concept represents the combined category."@en .

dpv-owl:IdentityAuthentication a rdfs:Class,
        owl:Class,
        dpv-owl:Purpose ;
    dct:contributor "Georg P. Krog, Harshvardhan J. Pandit, Beatriz Esteves" ;
    dct:created "2024-04-14"^^xsd:date ;
    rdfs:isDefinedBy dpv-owl: ;
    rdfs:subClassOf dpv-owl:EnforceSecurity ;
    sw:term_status "accepted"@en ;
    skos:definition "Purposes associated with performing authentication based on identity as a form of security"@en ;
    skos:prefLabel "Identity Authentication"@en .

dpv-owl:IdentityManagementMethod a rdfs:Class,
        owl:Class,
        dpv-owl:OrganisationalMeasure ;
    dct:contributor "Harshvardhan J. Pandit" ;
    dct:created "2022-08-17"^^xsd:date ;
    dct:source [ a schema:WebPage ;
            schema:name "ENISA Reference Incident Classification Taxonomy 2018" ;
            schema:url "https://www.enisa.europa.eu/publications/reference-incident-classification-taxonomy/" ] ;
    rdfs:isDefinedBy dpv-owl: ;
    rdfs:subClassOf dpv-owl:AuthorisationProcedure ;
    sw:term_status "accepted"@en ;
    skos:definition "Management of identity and identity-based processes"@en ;
    skos:prefLabel "Identity Management Method"@en .

dpv-owl:IdentityVerification a rdfs:Class,
        owl:Class,
        dpv-owl:Purpose ;
    dct:contributor "Harshvardhan J. Pandit, Javier Fernández, Axel Polleres, Elmar Kiesling, Fajar Ekaputra, Simon Steyskal" ;
    dct:created "2019-04-05"^^xsd:date ;
    rdfs:isDefinedBy dpv-owl: ;
    rdfs:subClassOf dpv-owl:Verification ;
    sw:term_status "accepted"@en ;
    skos:definition "Purposes associated with verifying or authenticating identity as a form of security"@en ;
    skos:prefLabel "Identity Verification"@en .

dpv-owl:Immigrant a rdfs:Class,
        owl:Class,
        dpv-owl:DataSubject ;
    dct:contributor "Harshvardhan J. Pandit, Georg P. Krog, Julian Flake, Paul Ryan, Beatriz Esteves" ;
    dct:created "2022-04-06"^^xsd:date ;
    rdfs:isDefinedBy dpv-owl: ;
    rdfs:subClassOf dpv-owl:DataSubject ;
    sw:term_status "accepted"@en ;
    skos:definition "Data subjects that are immigrants (for a jurisdiction)"@en ;
    skos:prefLabel "Immigrant"@en .

dpv-owl:Impact a rdfs:Class,
        owl:Class ;
    dct:contributor "Harshvardhan J. Pandit, Julian Flake, Georg P. Krog, Fajar Ekaputra, Beatriz Esteves" ;
    dct:created "2022-03-23"^^xsd:date ;
    vann:example dex-owl:E0027,
        dex-owl:E0068,
        dex-owl:E0069 ;
    rdfs:isDefinedBy dpv-owl: ;
    rdfs:subClassOf dpv-owl:Consequence ;
    sw:term_status "accepted"@en ;
    skos:definition "The impact(s) possible or arising as a consequence from specified context"@en ;
    skos:prefLabel "Impact"@en ;
    skos:scopeNote "Impact is a stronger notion of consequence in terms of influence, change, or effect on something e.g. for impact assessments"@en .

dpv-owl:ImpactAssessment a rdfs:Class,
        owl:Class,
        dpv-owl:OrganisationalMeasure ;
    dct:contributor "Georg P. Krog, Harshvardhan J. Pandit, Paul Ryan" ;
    dct:created "2020-11-04"^^xsd:date ;
    rdfs:isDefinedBy dpv-owl: ;
    rdfs:subClassOf dpv-owl:RiskAssessment ;
    sw:term_status "accepted"@en ;
    skos:definition "Calculating or determining the likelihood of impact of an existing or proposed process, which can involve risks or detriments."@en ;
    skos:prefLabel "Impact Assessment"@en .

dpv-owl:ImpliedConsent a rdfs:Class,
        owl:Class,
        dpv-owl:LegalBasis ;
    dct:contributor "Georg P. Krog, Harshvardhan J. Pandit, Paul Ryan, Julian Flake" ;
    dct:created "2022-06-21"^^xsd:date ;
    rdfs:isDefinedBy dpv-owl: ;
    rdfs:subClassOf dpv-owl:InformedConsent ;
    sw:term_status "accepted"@en ;
    skos:definition "Consent that is implied indirectly through an action not associated solely with conveying a consenting decision"@en ;
    skos:prefLabel "Implied Consent"@en ;
    skos:scopeNote "Implied consent is expected to also be Informed Consent. An example is a CCTV notice outside a monitored area that informs the individuals that by walking in they would be consenting to the use of camera for surveillance."@en .

dpv-owl:Importance a rdfs:Class,
        owl:Class ;
    dct:contributor "Harshvardhan J. Pandit, Paul Ryan, Georg P. Krog, Julian Flake, Beatriz Esteves" ;
    dct:created "2022-02-09"^^xsd:date ;
    rdfs:isDefinedBy dpv-owl: ;
    rdfs:subClassOf dpv-owl:Context ;
    sw:term_status "accepted"@en ;
    skos:definition "An indication of 'importance' within a context"@en ;
    skos:prefLabel "Importance"@en ;
    skos:scopeNote "Importance can be used to express importance, desirability, relevance, or significance as a context."@en .

dpv-owl:ImproveExistingProductsAndServices a rdfs:Class,
        owl:Class,
        dpv-owl:Purpose ;
    dct:contributor "Harshvardhan J. Pandit, Javier Fernández, Axel Polleres, Elmar Kiesling, Fajar Ekaputra, Simon Steyskal" ;
    dct:created "2019-04-05"^^xsd:date ;
    rdfs:isDefinedBy dpv-owl: ;
    rdfs:subClassOf dpv-owl:OptimisationForController ;
    sw:term_status "accepted"@en ;
    skos:definition "Purposes associated with improving existing products and services"@en ;
    skos:prefLabel "Improve Existing Products and Services"@en .

dpv-owl:ImproveHealthcare a rdfs:Class,
        owl:Class,
        dpv-owl:Purpose ;
    dct:contributor "Beatriz Esteves, Harshvardhan J. Pandit" ;
    dct:created "2024-02-14"^^xsd:date ;
    dct:source "DGA 2.16"@en ;
    rdfs:isDefinedBy dpv-owl: ;
    rdfs:subClassOf dpv-owl:PublicBenefit ;
    sw:term_status "accepted"@en ;
    skos:definition "Purposes associated with improving healthcare systems such as for personalised treatments and curing chronic diseases"@en ;
    skos:prefLabel "Improve Healthcare"@en .

dpv-owl:ImproveInternalCRMProcesses a rdfs:Class,
        owl:Class,
        dpv-owl:Purpose ;
    dct:contributor "Harshvardhan J. Pandit, Javier Fernández, Axel Polleres, Elmar Kiesling, Fajar Ekaputra, Simon Steyskal" ;
    dct:created "2019-04-05"^^xsd:date ;
    rdfs:isDefinedBy dpv-owl: ;
    rdfs:subClassOf dpv-owl:CustomerRelationshipManagement,
        dpv-owl:OptimisationForController ;
    sw:term_status "accepted"@en ;
    skos:definition "Purposes associated with improving customer-relationship management (CRM) processes"@en ;
    skos:prefLabel "Improve Internal CRM Processes"@en .

dpv-owl:ImprovePublicServices a rdfs:Class,
        owl:Class,
        dpv-owl:Purpose ;
    dct:contributor "Beatriz Esteves, Harshvardhan J. Pandit" ;
    dct:created "2024-02-14"^^xsd:date ;
    dct:source "DGA 2.16"@en ;
    rdfs:isDefinedBy dpv-owl: ;
    rdfs:subClassOf dpv-owl:PublicBenefit ;
    sw:term_status "accepted"@en ;
    skos:definition "Purposes associated with improving the provision of public services, such as public safety, education or law enforcement"@en ;
    skos:prefLabel "Improve Public Services"@en .

dpv-owl:ImproveTransportMobility a rdfs:Class,
        owl:Class,
        dpv-owl:Purpose ;
    dct:contributor "Beatriz Esteves, Harshvardhan J. Pandit" ;
    dct:created "2024-02-14"^^xsd:date ;
    dct:source "DGA 2.16"@en ;
    rdfs:isDefinedBy dpv-owl: ;
    rdfs:subClassOf dpv-owl:PublicBenefit ;
    sw:term_status "accepted"@en ;
    skos:definition "Purposes associated with improving traffic, public transport systems or costs for drivers"@en ;
    skos:prefLabel "Improve Transport and Mobility"@en .

dpv-owl:IncidentManagementProcedures a rdfs:Class,
        owl:Class,
        dpv-owl:OrganisationalMeasure ;
    dct:contributor "Harshvardhan J. Pandit" ;
    dct:created "2022-08-17"^^xsd:date ;
    dct:source [ a schema:WebPage ;
            schema:name "ENISA 5G Cybersecurity Standards" ;
            schema:url "https://www.enisa.europa.eu/publications/5g-cybersecurity-standards" ] ;
    rdfs:isDefinedBy dpv-owl: ;
    rdfs:subClassOf dpv-owl:GovernanceProcedures ;
    sw:term_status "accepted"@en ;
    skos:definition "Procedures related to management of incidents"@en ;
    skos:prefLabel "Incident Management Procedures"@en .

dpv-owl:IncidentReportingCommunication a rdfs:Class,
        owl:Class,
        dpv-owl:OrganisationalMeasure ;
    dct:contributor "Harshvardhan J. Pandit" ;
    dct:created "2022-08-17"^^xsd:date ;
    dct:source [ a schema:WebPage ;
            schema:name "ENISA 5G Cybersecurity Standards" ;
            schema:url "https://www.enisa.europa.eu/publications/5g-cybersecurity-standards" ] ;
    rdfs:isDefinedBy dpv-owl: ;
    rdfs:subClassOf dpv-owl:GovernanceProcedures ;
    sw:term_status "accepted"@en ;
    skos:definition "Procedures related to management of incident reporting"@en ;
    skos:prefLabel "Incident Reporting Communication"@en .

dpv-owl:IncorrectData a rdfs:Class,
        owl:Class ;
    dct:contributor "Harshvardhan J. Pandit" ;
    dct:created "2022-11-02"^^xsd:date ;
    rdfs:isDefinedBy dpv-owl: ;
    rdfs:subClassOf dpv-owl:Data ;
    sw:term_status "accepted"@en ;
    skos:definition "Data that is known to be incorrect or inconsistent with some requirements"@en ;
    skos:prefLabel "Incorrect Data"@en .

dpv-owl:IncreaseServiceRobustness a rdfs:Class,
        owl:Class,
        dpv-owl:Purpose ;
    dct:contributor "Harshvardhan J. Pandit, Javier Fernández, Axel Polleres, Elmar Kiesling, Fajar Ekaputra, Simon Steyskal" ;
    dct:created "2019-04-05"^^xsd:date ;
    rdfs:isDefinedBy dpv-owl: ;
    rdfs:subClassOf dpv-owl:OptimisationForController ;
    sw:term_status "accepted"@en ;
    skos:definition "Purposes associated with improving robustness and resilience of services"@en ;
    skos:prefLabel "Increase Service Robustness"@en .

dpv-owl:IndeterminateDuration a rdfs:Class,
        owl:Class,
        dpv-owl:Duration ;
    dct:contributor "Harshvardhan J. Pandit" ;
    dct:created "2022-11-30"^^xsd:date ;
    rdfs:isDefinedBy dpv-owl: ;
    rdfs:subClassOf dpv-owl:Duration ;
    sw:term_status "accepted"@en ;
    skos:definition "Duration that is indeterminate or cannot be determined"@en ;
    skos:prefLabel "Indeterminate Duration"@en ;
    skos:scopeNote "Indeterminate means (exact or otherwise) information about the duration cannot be determined, which is distinct from 'EndlessDuration' where it is known (or decided) that the duration is open-ended or without an end."@en .

dpv-owl:IndustryConsortium a rdfs:Class,
        owl:Class ;
    dct:contributor "Harshvardhan J. Pandit" ;
    dct:created "2022-02-02"^^xsd:date ;
    dct:modified "2020-10-05"^^xsd:date ;
    dct:source [ a schema:WebPage ;
            schema:name "ADMS controlled vocabulary" ;
            schema:url "http://purl.org/adms" ] ;
    rdfs:isDefinedBy dpv-owl: ;
    rdfs:subClassOf dpv-owl:Organisation ;
    sw:term_status "accepted"@en ;
    skos:definition "A consortium established and comprising on industry organisations"@en ;
    skos:prefLabel "Industry Consortium"@en .

dpv-owl:Infer a rdfs:Class,
        owl:Class,
        dpv-owl:Processing ;
    dct:contributor "Harshvardhan J. Pandit" ;
    dct:created "2022-04-20"^^xsd:date ;
    dct:modified "2022-10-14"^^xsd:date ;
    vann:example dex-owl:E0009 ;
    rdfs:isDefinedBy dpv-owl: ;
    rdfs:subClassOf dpv-owl:Derive ;
    sw:term_status "accepted"@en ;
    skos:definition "to infer data from existing data"@en ;
    skos:prefLabel "Infer"@en ;
    skos:scopeNote "Infer indicates data that is derived without it being present or obtainable from existing data. For data that is presented, and is 'extracted' or 'obtained' from existing data, see Derive."@en .

dpv-owl:InferredData a rdfs:Class,
        owl:Class ;
    dct:created "2023-12-10"^^xsd:date ;
    rdfs:isDefinedBy dpv-owl: ;
    rdfs:subClassOf dpv-owl:DerivedData ;
    sw:term_status "accepted"@en ;
    skos:definition "Data that has been obtained through inferences of other data"@en ;
    skos:prefLabel "Inferred Data"@en .

dpv-owl:InferredPersonalData a rdfs:Class,
        owl:Class ;
    dct:contributor "Harshvardhan J. Pandit" ;
    dct:created "2022-01-19"^^xsd:date ;
    dct:modified "2023-12-10"^^xsd:date ;
    vann:example dex-owl:E0009 ;
    rdfs:isDefinedBy dpv-owl: ;
    rdfs:subClassOf dpv-owl:DerivedPersonalData,
        dpv-owl:InferredData ;
    sw:term_status "accepted"@en ;
    skos:definition "Personal Data that is obtained through inference from other data"@en ;
    skos:prefLabel "Inferred Personal Data"@en ;
    skos:scopeNote "Inferred Data is derived data generated from existing data, but which did not originally exist within it, e.g. inferring demographics from browsing history."@en .

dpv-owl:InformationFlowControl a rdfs:Class,
        owl:Class,
        dpv-owl:TechnicalMeasure ;
    dct:contributor "Harshvardhan J. Pandit" ;
    dct:created "2022-08-17"^^xsd:date ;
    dct:source [ a schema:WebPage ;
            schema:name "ENISA Reference Incident Classification Taxonomy 2018" ;
            schema:url "https://www.enisa.europa.eu/publications/reference-incident-classification-taxonomy/" ] ;
    rdfs:isDefinedBy dpv-owl: ;
    rdfs:subClassOf dpv-owl:TechnicalMeasure ;
    sw:term_status "accepted"@en ;
    skos:definition "Use of measures to control information flows"@en ;
    skos:prefLabel "Information Flow Control"@en .

dpv-owl:InformationSecurityPolicy a rdfs:Class,
        owl:Class,
        dpv-owl:OrganisationalMeasure ;
    dct:contributor "Harshvardhan J. Pandit" ;
    dct:created "2022-08-17"^^xsd:date ;
    dct:modified "2024-04-14"^^xsd:date ;
    dct:source [ a schema:WebPage ;
            schema:name "ENISA 5G Cybersecurity Standards" ;
            schema:url "https://www.enisa.europa.eu/publications/5g-cybersecurity-standards" ] ;
    rdfs:isDefinedBy dpv-owl: ;
    rdfs:subClassOf dpv-owl:Policy ;
    sw:term_status "accepted"@en ;
    skos:definition "Policy regarding security of information"@en ;
    skos:prefLabel "Information Security Policy"@en .

dpv-owl:InformedConsent a rdfs:Class,
        owl:Class,
        dpv-owl:LegalBasis ;
    dct:contributor "Georg P. Krog, Harshvardhan J. Pandit, Paul Ryan, Julian Flake" ;
    dct:created "2022-06-21"^^xsd:date ;
    rdfs:isDefinedBy dpv-owl: ;
    rdfs:subClassOf dpv-owl:Consent ;
    sw:term_status "accepted"@en ;
    skos:definition "Consent that is informed i.e. with the requirement to provide sufficient information to make a consenting decision"@en ;
    skos:prefLabel "Informed Consent"@en ;
    skos:scopeNote "The specifics for what information should be provided or made available will depend on the context, use-case, or relevant legal requirements"@en .

dpv-owl:InnovativeUseOfExistingTechnology a rdfs:Class,
        owl:Class,
        dpv-owl:InnovativeUseOfTechnology ;
    dct:created "2023-12-10"^^xsd:date ;
    rdfs:isDefinedBy dpv-owl: ;
    rdfs:subClassOf dpv-owl:InnovativeUseOfTechnology ;
    sw:term_status "accepted"@en ;
    skos:definition "Involvement of existing technologies used in an innovative manner"@en ;
    skos:prefLabel "Innovative Use of Existing Technologies"@en .

dpv-owl:InnovativeUseOfNewTechnologies a rdfs:Class,
        owl:Class,
        dpv-owl:InnovativeUseOfTechnology ;
    dct:contributor "Harshvardhan J. Pandit, Piero Bonatti" ;
    dct:created "2020-11-04"^^xsd:date ;
    dct:modified "2023-12-10"^^xsd:date ;
    dct:source [ a schema:WebPage ;
            schema:name "GDPR Art.4-2" ;
            schema:url "https://eur-lex.europa.eu/eli/reg/2016/679/art_4/par_2/oj" ] ;
    rdfs:isDefinedBy dpv-owl: ;
    rdfs:subClassOf dpv-owl:InnovativeUseOfTechnology ;
    sw:term_status "accepted"@en ;
    skos:definition "Involvement of a new (innovative) technologies"@en ;
    skos:prefLabel "Innovative Use of New Technologies"@en ;
    skos:scopeNote "New technologies are by definition considered innovative"@en .

dpv-owl:InnovativeUseOfTechnology a rdfs:Class,
        owl:Class ;
    dct:created "2023-12-10"^^xsd:date ;
    rdfs:isDefinedBy dpv-owl: ;
    rdfs:subClassOf dpv-owl:ProcessingContext ;
    sw:term_status "accepted"@en ;
    skos:definition "Indicates that technology is being used in an innovative manner"@en ;
    skos:prefLabel "Innovative use of Technology"@en ;
    skos:scopeNote "Innovative here refers to 'state of the art' rather than the implementing entity, and can be for either new technology or new uses of existing technology"@en .

dpv-owl:IntellectualPropertyData a rdfs:Class,
        owl:Class ;
    dct:created "2024-02-14"^^xsd:date ;
    dct:source "DGA 5.10"@en ;
    rdfs:isDefinedBy dpv-owl: ;
    rdfs:subClassOf dpv-owl:ConfidentialData ;
    sw:term_status "accepted"@en ;
    skos:definition "Data protected by Intellectual Property rights and regulations"@en ;
    skos:prefLabel "Intellectual Property Data"@en .

dpv-owl:Intended a rdfs:Class,
        owl:Class,
        dpv-owl:IntentionStatus ;
    dct:contributor "Harshvardhan J. Pandit, Delaram Golpayegani, Georg P. Krog, Paul Ryan" ;
    dct:created "2024-05-10"^^xsd:date ;
    rdfs:isDefinedBy dpv-owl: ;
    rdfs:subClassOf dpv-owl:IntentionStatus ;
    sw:term_status "accepted"@en ;
    skos:definition "Status indicating the specified context was intended"@en ;
    skos:prefLabel "Intended"@en .

dpv-owl:IntentionStatus a rdfs:Class,
        owl:Class ;
    dct:contributor "Harshvardhan J. Pandit, Delaram Golpayegani, Georg P. Krog, Paul Ryan" ;
    dct:created "2024-05-10"^^xsd:date ;
    rdfs:isDefinedBy dpv-owl: ;
    rdfs:subClassOf dpv-owl:Status ;
    sw:term_status "accepted"@en ;
    skos:definition "Status indicating whether the specified context was intended or unintended"@en ;
    skos:prefLabel "Intention Status"@en ;
    skos:scopeNote "Intention is associated with the goal or purpose for what is about to happen i.e. an ex-ante indication of whether the specified context is/was planned or intended. Intention and Expectation are closely related terms. We recommend using Intention when the entity has the ability to control the implementation and Expectation for when the entity does not have control or for what happens after or beyond the exercise of control."@en .

dpv-owl:InternalResourceOptimisation a rdfs:Class,
        owl:Class,
        dpv-owl:Purpose ;
    dct:contributor "Harshvardhan J. Pandit, Javier Fernández, Axel Polleres, Elmar Kiesling, Fajar Ekaputra, Simon Steyskal" ;
    dct:created "2019-04-05"^^xsd:date ;
    rdfs:isDefinedBy dpv-owl: ;
    rdfs:subClassOf dpv-owl:OptimisationForController ;
    sw:term_status "accepted"@en ;
    skos:definition "Purposes associated with optimisation of internal resource availability and usage for organisation"@en ;
    skos:prefLabel "Internal Resource Optimisation"@en .

dpv-owl:InternationalOrganisation a rdfs:Class,
        owl:Class ;
    dct:contributor "Julian Flake, Georg P. Krog" ;
    dct:created "2022-03-23"^^xsd:date ;
    dct:modified "2020-10-05"^^xsd:date ;
    dct:source [ a schema:WebPage ;
            schema:name "GDPR Art.4-26" ;
            schema:url "https://eur-lex.europa.eu/eli/reg/2016/679/art_4/par_26/oj" ] ;
    rdfs:isDefinedBy dpv-owl: ;
    rdfs:subClassOf dpv-owl:Organisation ;
    sw:term_status "accepted"@en ;
    skos:definition "An organisation and its subordinate bodies governed by public international law, or any other body which is set up by, or on the basis of, an agreement between two or more countries"@en ;
    skos:prefLabel "International Organisation"@en .

dpv-owl:IntrusionDetectionSystem a rdfs:Class,
        owl:Class,
        dpv-owl:TechnicalMeasure ;
    dct:contributor "Harshvardhan J. Pandit" ;
    dct:created "2022-08-17"^^xsd:date ;
    dct:source [ a schema:WebPage ;
            schema:name "ENISA Reference Incident Classification Taxonomy 2018" ;
            schema:url "https://www.enisa.europa.eu/publications/reference-incident-classification-taxonomy/" ] ;
    rdfs:isDefinedBy dpv-owl: ;
    rdfs:subClassOf dpv-owl:SecurityMethod ;
    sw:term_status "accepted"@en ;
    skos:definition "Use of measures to detect intrusions and other unauthorised attempts to gain access to a system"@en ;
    skos:prefLabel "Intrusion Detection System"@en .

dpv-owl:InvolvementStatus a rdfs:Class,
        owl:Class ;
    dct:contributor "Harshvardhan J. Pandit, Delaram Golpayegani, Georg P. Krog, Paul Ryan" ;
    dct:created "2024-05-10"^^xsd:date ;
    rdfs:isDefinedBy dpv-owl: ;
    rdfs:subClassOf dpv-owl:Status ;
    sw:term_status "accepted"@en ;
    skos:definition "Status indicating whether the involvement of specified context"@en ;
    skos:prefLabel "Involvement Status"@en .

dpv-owl:JobApplicant a rdfs:Class,
        owl:Class,
        dpv-owl:DataSubject ;
    dct:contributor "Harshvardhan J. Pandit, Georg P. Krog, Julian Flake, Paul Ryan, Beatriz Esteves" ;
    dct:created "2022-04-06"^^xsd:date ;
    rdfs:isDefinedBy dpv-owl: ;
    rdfs:subClassOf dpv-owl:DataSubject ;
    sw:term_status "accepted"@en ;
    skos:definition "Data subjects that apply for jobs or employments"@en ;
    skos:prefLabel "Job Applicant"@en .

dpv-owl:JointDataControllers a rdfs:Class,
        owl:Class ;
    dct:contributor "Georg P. Krog, Harshvardhan J. Pandit" ;
    dct:created "2022-02-02"^^xsd:date ;
    rdfs:isDefinedBy dpv-owl: ;
    rdfs:subClassOf dpv-owl:DataController ;
    sw:term_status "accepted"@en ;
    skos:definition "A group of Data Controllers that jointly determine the purposes and means of processing"@en ;
    skos:prefLabel "Joint Data Controllers"@en ;
    skos:scopeNote "While Joint Data Controllers operate together, they are made up of individually distinct legal entities. To indicate the membership of this group, hasDataController should be used to denote each Data Controller. The concept of Joint Data Controllers also allows specifying a single group as the 'Controller' and to specify role and responsibilities within that group for each entity using DPV's concepts (e.g. isImplementedByEntity)"@en .

dpv-owl:JointDataControllersAgreement a rdfs:Class,
        owl:Class,
        dpv-owl:LegalMeasure ;
    dct:contributor "Georg P. Krog, Harshvardhan J. Pandit, Beatriz Esteves, Paul Ryan, Julian Flake" ;
    dct:created "2022-01-26"^^xsd:date ;
    rdfs:isDefinedBy dpv-owl: ;
    rdfs:subClassOf dpv-owl:DataProcessingAgreement ;
    sw:term_status "accepted"@en ;
    skos:definition "An agreement outlining conditions, criteria, obligations, responsibilities, and specifics for carrying out processing of data between Controllers within a Joint Controllers relationship"@en ;
    skos:prefLabel "Joint Data Controllers Agreement"@en .

dpv-owl:Justification a rdfs:Class,
        owl:Class ;
    dct:contributor "Harshvardhan J. Pandit" ;
    dct:created "2022-06-15"^^xsd:date ;
    vann:example dex-owl:E0057,
        dex-owl:E0058,
        dex-owl:E0059,
        dex-owl:E0061,
        dex-owl:E0062,
        dex-owl:E0063 ;
    rdfs:isDefinedBy dpv-owl: ;
    rdfs:subClassOf dpv-owl:Context ;
    sw:term_status "accepted"@en ;
    skos:definition "A form of documentation providing reasons, explanations, or justifications"@en ;
    skos:prefLabel "Justification"@en .

dpv-owl:LargeDataVolume a rdfs:Class,
        owl:Class,
        dpv-owl:DataVolume ;
    dct:contributor "Harshvardhan J. Pandit" ;
    dct:created "2022-06-15"^^xsd:date ;
    rdfs:isDefinedBy dpv-owl: ;
    rdfs:subClassOf dpv-owl:DataVolume ;
    sw:term_status "accepted"@en ;
    skos:definition "Data volume that is considered large within the context"@en ;
    skos:prefLabel "Large Data Volume"@en .

dpv-owl:LargeScaleOfDataSubjects a rdfs:Class,
        owl:Class,
        dpv-owl:DataSubjectScale ;
    dct:contributor "Harshvardhan J. Pandit" ;
    dct:created "2022-06-15"^^xsd:date ;
    rdfs:isDefinedBy dpv-owl: ;
    rdfs:subClassOf dpv-owl:DataSubjectScale ;
    sw:term_status "accepted"@en ;
    skos:definition "Scale of data subjects considered large within the context"@en ;
    skos:prefLabel "Large Scale Of Data Subjects"@en .

dpv-owl:LargeScaleProcessing a rdfs:Class,
        owl:Class,
        dpv-owl:ProcessingScale ;
    dct:contributor "Harshvardhan J. Pandit, Piero Bonatti" ;
    dct:created "2020-11-04"^^xsd:date ;
    dct:modified "2022-09-07"^^xsd:date ;
    dct:source [ a schema:WebPage ;
            schema:name "GDPR Art.4-2" ;
            schema:url "https://eur-lex.europa.eu/eli/reg/2016/679/art_4/par_2/oj" ] ;
    rdfs:isDefinedBy dpv-owl: ;
    rdfs:subClassOf dpv-owl:ProcessingScale ;
    sw:term_status "accepted"@en ;
    skos:definition "Processing that takes place at large scales (as specified by some criteria)"@en ;
    skos:prefLabel "Large Scale Processing"@en ;
    skos:scopeNote "The exact definition of what constitutes \"large scale\" depends on use of jurisdictional, domain-specific, or other forms of externally defined criterias. Where possible, this should be reflected by extending this term with the appropriate context."@en .

dpv-owl:Law a rdfs:Class,
        owl:Class ;
    dct:contributor "Harshvardhan J. Pandit" ;
    dct:created "2022-01-19"^^xsd:date ;
    rdfs:isDefinedBy dpv-owl: ;
    rdfs:subClassOf rdfs:Class ;
    sw:term_status "accepted"@en ;
    skos:definition "A law is a set of rules created by government or authorities"@en ;
    skos:prefLabel "Law"@en .

dpv-owl:Lawful a rdfs:Class,
        owl:Class,
        dpv-owl:Lawfulness ;
    dct:contributor "Harshvardhan J. Pandit" ;
    dct:created "2022-10-19"^^xsd:date ;
    rdfs:isDefinedBy dpv-owl: ;
    rdfs:subClassOf dpv-owl:Lawfulness ;
    sw:term_status "accepted"@en ;
    skos:definition "State of being lawful or legally compliant"@en ;
    skos:prefLabel "Lawful"@en .

dpv-owl:Lawfulness a rdfs:Class,
        owl:Class ;
    dct:contributor "Harshvardhan J. Pandit" ;
    dct:created "2022-10-19"^^xsd:date ;
    rdfs:isDefinedBy dpv-owl: ;
    rdfs:subClassOf dpv-owl:ComplianceStatus ;
    sw:term_status "accepted"@en ;
    skos:definition "Status associated with expressing lawfulness or legal compliance"@en ;
    skos:prefLabel "Lawfulness"@en .

dpv-owl:LawfulnessUnkown a rdfs:Class,
        owl:Class,
        dpv-owl:Lawfulness ;
    dct:contributor "Harshvardhan J. Pandit" ;
    dct:created "2022-10-19"^^xsd:date ;
    rdfs:isDefinedBy dpv-owl: ;
    rdfs:subClassOf dpv-owl:Lawfulness ;
    sw:term_status "accepted"@en ;
    skos:definition "State of the lawfulness not being known"@en ;
    skos:prefLabel "Lawfulness Unknown"@en .

dpv-owl:LegalAgreement a rdfs:Class,
        owl:Class,
        dpv-owl:LegalMeasure ;
    dct:contributor "Axel Polleres, Rob Brennan, Harshvardhan J. Pandit, Mark Lizar" ;
    dct:created "2019-04-05"^^xsd:date ;
    rdfs:isDefinedBy dpv-owl: ;
    rdfs:subClassOf dpv-owl:LegalMeasure ;
    sw:term_status "accepted"@en ;
    skos:definition "A legally binding agreement"@en ;
    skos:prefLabel "Legal Agreement"@en .

dpv-owl:LegalBasis a rdfs:Class,
        owl:Class ;
    dct:created "2019-04-05"^^xsd:date ;
    dct:modified "2020-11-04"^^xsd:date ;
    vann:example dex-owl:E0014 ;
    rdfs:isDefinedBy dpv-owl: ;
    sw:term_status "accepted"@en ;
    skos:definition "Legal basis used to justify processing of data or use of technology in accordance with a law"@en ;
    skos:prefLabel "Legal Basis"@en ;
    skos:scopeNote "Legal basis (plural: legal bases) are defined by legislations and regulations, whose applicability is usually restricted to specific jurisdictions which can be represented using dpv:hasJurisdiction or dpv:hasLaw. Legal basis can be used without such declarations, e.g. 'Consent', however their interpretation will require association with a law, e.g. 'EU GDPR'."@en .

dpv-owl:LegalCompliance a rdfs:Class,
        owl:Class,
        dpv-owl:Purpose ;
    dct:contributor "Georg P. Krog, Harshvardhan J. Pandit, Beatriz Esteves" ;
    dct:created "2020-11-04"^^xsd:date ;
    dct:modified "2022-11-09"^^xsd:date ;
    rdfs:isDefinedBy dpv-owl: ;
    rdfs:subClassOf dpv-owl:FulfilmentOfObligation ;
    sw:term_status "accepted"@en ;
    skos:definition "Purposes associated with carrying out data processing to fulfill a legal or statutory obligation"@en ;
    skos:prefLabel "Legal Compliance"@en ;
    skos:scopeNote "This purpose only refers to processing that is additionally required in order to fulfill the obligations and requirements associated with a law. For example, the use of consent would have its own separate purposes, with this purpose addressing a legal requirement for maintaining consent record (along with RecordManagement). This purpose will typically be used with Legal Obligation as the legal basis."@en .

dpv-owl:LegalComplianceAssessment a rdfs:Class,
        owl:Class,
        dpv-owl:OrganisationalMeasure ;
    dct:contributor "Harshvardhan J. Pandit, Georg P. Krog" ;
    dct:created "2024-04-14"^^xsd:date ;
    rdfs:isDefinedBy dpv-owl: ;
    rdfs:subClassOf dpv-owl:ComplianceAssessment ;
    sw:term_status "accepted"@en ;
    skos:definition "Assessment regarding legal compliance"@en ;
    skos:prefLabel "Legal Compliance Assessment"@en .

dpv-owl:LegalEntity a rdfs:Class,
        owl:Class ;
    dct:contributor "Harshvardhan J. Pandit" ;
    dct:created "2019-04-05"^^xsd:date ;
    rdfs:isDefinedBy dpv-owl: ;
    rdfs:subClassOf dpv-owl:Entity ;
    sw:term_status "accepted"@en ;
    skos:definition "A human or non-human 'thing' that constitutes as an entity and which is recognised and defined in law"@en ;
    skos:prefLabel "Legal Entity"@en .

dpv-owl:LegalMeasure a rdfs:Class,
        owl:Class ;
    dct:created "2023-12-10"^^xsd:date ;
    dct:modified "2023-12-10"^^xsd:date ;
    dct:source "DGA 12.j"@en ;
    rdfs:isDefinedBy dpv-owl: ;
    rdfs:subClassOf dpv-owl:TechnicalOrganisationalMeasure ;
    sw:term_status "accepted"@en ;
    skos:definition "Legal measures used to safeguard and ensure good practices in connection with data and technologies"@en ;
    skos:prefLabel "Legal Measure"@en .

dpv-owl:LegalObligation a rdfs:Class,
        owl:Class,
        dpv-owl:LegalBasis ;
    dct:contributor "Harshvardhan J. Pandit" ;
    dct:created "2021-04-07"^^xsd:date ;
    vann:example dex-owl:E0042 ;
    rdfs:isDefinedBy dpv-owl: ;
    rdfs:subClassOf dpv-owl:LegalBasis ;
    sw:term_status "accepted"@en ;
    skos:definition "Legal Obligation to conduct the specified activities"@en ;
    skos:prefLabel "Legal Obligation"@en .

dpv-owl:LegitimateInterest a rdfs:Class,
        owl:Class,
        dpv-owl:LegalBasis ;
    dct:contributor "Harshvardhan J. Pandit" ;
    dct:created "2021-05-19"^^xsd:date ;
    vann:example dex-owl:E0065 ;
    rdfs:isDefinedBy dpv-owl: ;
    rdfs:subClassOf dpv-owl:LegalBasis ;
    sw:term_status "accepted"@en ;
    skos:definition "Legitimate Interests of a Party as justification for specified activities"@en ;
    skos:prefLabel "Legitimate Interest"@en .

dpv-owl:LegitimateInterestAssessment a rdfs:Class,
        owl:Class,
        dpv-owl:OrganisationalMeasure ;
    dct:contributor "Georg P. Krog, Harshvardhan J. Pandit, Paul Ryan" ;
    dct:created "2021-09-08"^^xsd:date ;
    rdfs:isDefinedBy dpv-owl: ;
    rdfs:subClassOf dpv-owl:Assessment ;
    sw:term_status "accepted"@en ;
    skos:definition "Indicates an assessment regarding the use of legitimate interest as a lawful basis by the data controller"@en ;
    skos:prefLabel "Legitimate Interest Assessment"@en .

dpv-owl:LegitimateInterestOfController a rdfs:Class,
        owl:Class,
        dpv-owl:LegalBasis ;
    dct:contributor "Georg P. Krog, Harshvardhan J. Pandit, Paul Ryan" ;
    dct:created "2021-05-19"^^xsd:date ;
    vann:example dex-owl:E0065 ;
    rdfs:isDefinedBy dpv-owl: ;
    rdfs:subClassOf dpv-owl:LegitimateInterest ;
    sw:term_status "accepted"@en ;
    skos:definition "Legitimate Interests of a Data Controller in conducting specified activities"@en ;
    skos:prefLabel "Legitimate Interest of Controller"@en .

dpv-owl:LegitimateInterestOfDataSubject a rdfs:Class,
        owl:Class,
        dpv-owl:LegalBasis ;
    dct:contributor "Georg P. Krog" ;
    dct:created "2022-10-22"^^xsd:date ;
    rdfs:isDefinedBy dpv-owl: ;
    rdfs:subClassOf dpv-owl:LegitimateInterest ;
    sw:term_status "accepted"@en ;
    skos:definition "Legitimate Interests of the Data Subject in conducting specified activities"@en ;
    skos:prefLabel "Legitimate Interest of Data Subject"@en .

dpv-owl:LegitimateInterestOfThirdParty a rdfs:Class,
        owl:Class,
        dpv-owl:LegalBasis ;
    dct:contributor "Georg P. Krog, Harshvardhan J. Pandit, Paul Ryan" ;
    dct:created "2021-05-19"^^xsd:date ;
    rdfs:isDefinedBy dpv-owl: ;
    rdfs:subClassOf dpv-owl:LegitimateInterest ;
    sw:term_status "accepted"@en ;
    skos:definition "Legitimate Interests of a Third Party in conducting specified activities"@en ;
    skos:prefLabel "Legitimate Interest of Third Party"@en .

dpv-owl:Licence a rdfs:Class,
        owl:Class,
        dpv-owl:LegalMeasure ;
    dct:contributor "Beatriz Esteves, Harshvardhan J. Pandit" ;
    dct:created "2022-02-09"^^xsd:date ;
    dct:source "DGA 2.10"@en ;
    rdfs:isDefinedBy dpv-owl: ;
    rdfs:subClassOf dpv-owl:ContractualTerms ;
    sw:term_status "accepted"@en ;
    skos:definition "A Legal Document providing permission to utilise data or resource and outlining the conditions under which such use is considered valid"@en ;
    skos:prefLabel "Licence"@en ;
    skos:related odrl:Offer .

dpv-owl:Likelihood a rdfs:Class,
        owl:Class ;
    dct:contributor "Harshvardhan J. Pandit" ;
    dct:created "2022-07-22"^^xsd:date ;
    vann:example dex-owl:E0068 ;
    rdfs:isDefinedBy dpv-owl: ;
    sw:term_status "accepted"@en ;
    skos:definition "The likelihood or probability or chance of something taking place or occuring"@en ;
    skos:prefLabel "Likelihood"@en ;
    skos:scopeNote "Likelihood can be expressed in a subjective manner, such as 'Unlikely', or in a quantitative manner such as \"Twice in a Day\" (frequency per period). The suggestion is to use quantitative values, or to associate them with subjective terms used so as to enable accurate interpretations and interoperability. See the concepts related to Frequency and Duration for possible uses as a combination to express Likelihood."@en .

dpv-owl:LocalEnvironmentScale a rdfs:Class,
        owl:Class,
        dpv-owl:GeographicCoverage ;
    dct:contributor "Harshvardhan J. Pandit" ;
    dct:created "2022-06-15"^^xsd:date ;
    rdfs:isDefinedBy dpv-owl: ;
    rdfs:subClassOf dpv-owl:GeographicCoverage ;
    sw:term_status "accepted"@en ;
    skos:definition "Geographic coverage spanning a specific environment within the locality"@en ;
    skos:prefLabel "Local Environment Scale"@en ;
    skos:scopeNote "For example, geographic scale of an event take place in a specific building or room"@en .

dpv-owl:LocalLocation a rdfs:Class,
        owl:Class,
        dpv-owl:Location ;
    dct:contributor "Harshvardhan J. Pandit" ;
    dct:created "2022-06-15"^^xsd:date ;
    dct:modified "2020-10-05"^^xsd:date ;
    rdfs:isDefinedBy dpv-owl: ;
    rdfs:subClassOf dpv-owl:LocationLocality ;
    sw:term_status "accepted"@en ;
    skos:definition "Location is local"@en ;
    skos:prefLabel "Local Location"@en .

dpv-owl:LocalityScale a rdfs:Class,
        owl:Class,
        dpv-owl:GeographicCoverage ;
    dct:contributor "Harshvardhan J. Pandit" ;
    dct:created "2022-06-15"^^xsd:date ;
    rdfs:isDefinedBy dpv-owl: ;
    rdfs:subClassOf dpv-owl:GeographicCoverage ;
    sw:term_status "accepted"@en ;
    skos:definition "Geographic coverage spanning a specific locality"@en ;
    skos:prefLabel "Locality Scale"@en ;
    skos:scopeNote "For example, geographic scale of a city or an area within a city"@en .

dpv-owl:Location a rdfs:Class,
        owl:Class ;
    dct:contributor "Harshvardhan J. Pandit, Georg P. Krog" ;
    dct:created "2022-01-19"^^xsd:date ;
    vann:example dex-owl:E0060 ;
    rdfs:isDefinedBy dpv-owl: ;
    rdfs:subClassOf rdfs:Class ;
    sw:term_status "accepted"@en ;
    skos:definition "A location is a position, site, or area where something is located"@en ;
    skos:prefLabel "Location"@en ;
    skos:scopeNote "Location may be geographic, physical, or virtual."@en .

dpv-owl:LocationFixture a rdfs:Class,
        owl:Class ;
    dct:contributor "Harshvardhan J. Pandit" ;
    dct:created "2022-06-15"^^xsd:date ;
    vann:example dex-owl:E0060 ;
    rdfs:isDefinedBy dpv-owl: ;
    rdfs:subClassOf rdfs:Class ;
    sw:term_status "accepted"@en ;
    skos:definition "The fixture of location refers to whether the location is fixed"@en ;
    skos:prefLabel "Location Fixture"@en .

dpv-owl:LocationLocality a rdfs:Class,
        owl:Class,
        dpv-owl:Location ;
    dct:contributor "Harshvardhan J. Pandit" ;
    dct:created "2022-06-15"^^xsd:date ;
    dct:modified "2022-10-04"^^xsd:date ;
    vann:example dex-owl:E0060 ;
    rdfs:isDefinedBy dpv-owl: ;
    rdfs:subClassOf dpv-owl:Location ;
    sw:term_status "accepted"@en ;
    skos:definition "Locality refers to whether the specified location is local within some context, e.g. for the user"@en ;
    skos:prefLabel "Location Locality"@en .

dpv-owl:LoggingPolicy a rdfs:Class,
        owl:Class,
        dpv-owl:OrganisationalMeasure ;
    dct:contributor "Harshvardhan J. Pandit" ;
    dct:created "2022-08-17"^^xsd:date ;
    dct:modified "2024-04-14"^^xsd:date ;
    dct:source [ a schema:WebPage ;
            schema:name "ENISA 5G Cybersecurity Standards" ;
            schema:url "https://www.enisa.europa.eu/publications/5g-cybersecurity-standards" ] ;
    rdfs:isDefinedBy dpv-owl: ;
    rdfs:subClassOf dpv-owl:Policy ;
    sw:term_status "accepted"@en ;
    skos:definition "Policy for logging of information"@en ;
    skos:prefLabel "Logging Policy"@en .

dpv-owl:MaintainCreditCheckingDatabase a rdfs:Class,
        owl:Class,
        dpv-owl:Purpose ;
    dct:contributor "Harshvardhan J. Pandit, Georg P. Krog" ;
    dct:created "2022-06-15"^^xsd:date ;
    rdfs:isDefinedBy dpv-owl: ;
    rdfs:subClassOf dpv-owl:CreditChecking ;
    sw:term_status "accepted"@en ;
    skos:definition "Purposes associated with maintaining a Credit Checking Database"@en ;
    skos:prefLabel "Maintain Credit Checking Database"@en .

dpv-owl:MaintainCreditRatingDatabase a rdfs:Class,
        owl:Class,
        dpv-owl:Purpose ;
    dct:contributor "Harshvardhan J. Pandit, Georg P. Krog" ;
    dct:created "2022-06-15"^^xsd:date ;
    rdfs:isDefinedBy dpv-owl: ;
    rdfs:subClassOf dpv-owl:CreditChecking ;
    sw:term_status "accepted"@en ;
    skos:definition "Purposes associated with maintaining a Credit Rating Database"@en ;
    skos:prefLabel "Maintain Credit Rating Database"@en .

dpv-owl:MaintainFraudDatabase a rdfs:Class,
        owl:Class,
        dpv-owl:Purpose ;
    dct:contributor "Harshvardhan J. Pandit, Georg P. Krog" ;
    dct:created "2022-06-15"^^xsd:date ;
    rdfs:isDefinedBy dpv-owl: ;
    rdfs:subClassOf dpv-owl:FraudPreventionAndDetection ;
    sw:term_status "accepted"@en ;
    skos:definition "Purposes associated with maintaining a database related to identifying and identified fraud risks and fraud incidents"@en ;
    skos:prefLabel "Maintain Fraud Database"@en .

dpv-owl:MakeAvailable a rdfs:Class,
        owl:Class,
        dpv-owl:Processing ;
    dct:created "2019-05-07"^^xsd:date ;
    dct:source [ a schema:WebPage ;
            schema:name "GDPR Art.4-2" ;
            schema:url "https://eur-lex.europa.eu/eli/reg/2016/679/art_4/par_2/oj" ] ;
    rdfs:isDefinedBy dpv-owl: ;
    rdfs:subClassOf dpv-owl:Disclose ;
    sw:term_status "accepted"@en ;
    skos:definition "to transform or publish data to be used"@en ;
    skos:prefLabel "Make Available"@en .

dpv-owl:Marketing a rdfs:Class,
        owl:Class,
        dpv-owl:Purpose ;
    dct:contributor "Georg P. Krog, Harshvardhan J. Pandit, Beatriz Esteves" ;
    dct:created "2020-11-04"^^xsd:date ;
    rdfs:isDefinedBy dpv-owl: ;
    rdfs:subClassOf dpv-owl:Purpose ;
    sw:term_status "accepted"@en ;
    skos:definition "Purposes associated with conducting marketing in relation to organisation or products or services e.g. promoting, selling, and distributing"@en ;
    skos:prefLabel "Marketing"@en ;
    skos:scopeNote "Was commercial interest, changed to consider Marketing a separate Purpose category by itself"@en .

dpv-owl:Match a rdfs:Class,
        owl:Class,
        dpv-owl:Processing ;
    dct:contributor "Harshvardhan J. Pandit" ;
    dct:created "2022-04-20"^^xsd:date ;
    dct:source [ a schema:WebPage ;
            schema:name "A29WP WP 248 rev.01 Guideliens on DPIA" ;
            schema:url "https://ec.europa.eu/newsroom/article29/items/611236" ] ;
    rdfs:isDefinedBy dpv-owl: ;
    rdfs:subClassOf dpv-owl:Use ;
    sw:term_status "accepted"@en ;
    skos:definition "to combine, compare, or match data from different sources"@en ;
    skos:prefLabel "Match"@en .

dpv-owl:MediumDataVolume a rdfs:Class,
        owl:Class,
        dpv-owl:DataVolume ;
    dct:contributor "Harshvardhan J. Pandit, Georg P. Krog, Paul Ryan" ;
    dct:created "2022-06-15"^^xsd:date ;
    rdfs:isDefinedBy dpv-owl: ;
    rdfs:subClassOf dpv-owl:DataVolume ;
    sw:term_status "accepted"@en ;
    skos:definition "Data volume that is considered medium i.e. neither large nor small within the context"@en ;
    skos:prefLabel "Medium Data Volume"@en .

dpv-owl:MediumScaleOfDataSubjects a rdfs:Class,
        owl:Class,
        dpv-owl:DataSubjectScale ;
    dct:contributor "Harshvardhan J. Pandit, Georg P. Krog, Paul Ryan" ;
    dct:created "2022-06-15"^^xsd:date ;
    rdfs:isDefinedBy dpv-owl: ;
    rdfs:subClassOf dpv-owl:DataSubjectScale ;
    sw:term_status "accepted"@en ;
    skos:definition "Scale of data subjects considered medium i.e. neither large nor small within the context"@en ;
    skos:prefLabel "Medium Scale Of Data Subjects"@en .

dpv-owl:MediumScaleProcessing a rdfs:Class,
        owl:Class,
        dpv-owl:ProcessingScale ;
    dct:contributor "Harshvardhan J. Pandit" ;
    dct:created "2022-09-07"^^xsd:date ;
    rdfs:isDefinedBy dpv-owl: ;
    rdfs:subClassOf dpv-owl:ProcessingScale ;
    sw:term_status "accepted"@en ;
    skos:definition "Processing that takes place at medium scales (as specified by some criteria)"@en ;
    skos:prefLabel "Medium Scale Processing"@en .

dpv-owl:Member a rdfs:Class,
        owl:Class,
        dpv-owl:DataSubject ;
    dct:contributor "Harshvardhan J. Pandit, Georg P. Krog, Julian Flake, Paul Ryan, Beatriz Esteves" ;
    dct:created "2022-04-06"^^xsd:date ;
    rdfs:isDefinedBy dpv-owl: ;
    rdfs:subClassOf dpv-owl:DataSubject ;
    sw:term_status "accepted"@en ;
    skos:definition "Data subjects that are members of a group, organisation, or other collectives"@en ;
    skos:prefLabel "Member"@en .

dpv-owl:MemberPartnerManagement a rdfs:Class,
        owl:Class,
        dpv-owl:Purpose ;
    dct:contributor "Paul Ryan, Georg P. Krog, David Hickey, Harshvardhan J. Pandit" ;
    dct:created "2021-09-01"^^xsd:date ;
    dct:source [ a schema:WebPage ;
            schema:name "Belgian DPA ROPA Template" ;
            schema:url "https://www.privacycommission.be/nl/model-voor-een-register-van-de-verwerkingsactiviteiten" ] ;
    rdfs:isDefinedBy dpv-owl: ;
    rdfs:subClassOf dpv-owl:OrganisationGovernance ;
    sw:term_status "accepted"@en ;
    skos:definition "Purposes associated with maintaining a registry of shareholders, members, or partners for governance, administration, and management functions"@en ;
    skos:prefLabel "Members and Partners Management"@en .

dpv-owl:MentallyVulnerableDataSubject a rdfs:Class,
        owl:Class,
        dpv-owl:DataSubject ;
    dct:contributor "Georg P. Krog" ;
    dct:created "2022-06-15"^^xsd:date ;
    rdfs:isDefinedBy dpv-owl: ;
    rdfs:subClassOf dpv-owl:VulnerableDataSubject ;
    sw:term_status "accepted"@en ;
    skos:definition "Data subjects that are considered mentally vulnerable"@en ;
    skos:prefLabel "Mentally Vulnerable Data Subject"@en .

dpv-owl:MessageAuthenticationCodes a rdfs:Class,
        owl:Class,
        dpv-owl:TechnicalMeasure ;
    dct:contributor "Harshvardhan J. Pandit" ;
    dct:created "2022-08-17"^^xsd:date ;
    dct:source [ a schema:WebPage ;
            schema:name "ENISA Reference Incident Classification Taxonomy 2018" ;
            schema:url "https://www.enisa.europa.eu/publications/reference-incident-classification-taxonomy/" ] ;
    rdfs:isDefinedBy dpv-owl: ;
    rdfs:subClassOf dpv-owl:CryptographicAuthentication ;
    sw:term_status "accepted"@en ;
    skos:definition "Use of cryptographic methods to authenticate messages"@en ;
    skos:prefLabel "Message Authentication Codes (MAC)"@en .

dpv-owl:MetadataManagement a rdfs:Class,
        owl:Class,
        dpv-owl:OrganisationalMeasure ;
    dct:contributor "Harshvardhan J. Pandit" ;
    dct:created "2024-04-14"^^xsd:date ;
    rdfs:isDefinedBy dpv-owl: ;
    rdfs:subClassOf dpv-owl:DataGovernance ;
    sw:term_status "accepted"@en ;
    skos:definition "Measures associated with management of metadata"@en ;
    skos:prefLabel "Metadata Management"@en ;
    skos:scopeNote "Examples of metadata management include assessing which metadata are required or being used by technology, assessing their potential inclusion as personal data, and implementing a metadata based solution to manage data"@en .

dpv-owl:MisusePreventionAndDetection a rdfs:Class,
        owl:Class,
        dpv-owl:Purpose ;
    dct:created "2024-05-09"^^xsd:date ;
    dct:source "DGA 22.1(a)"@en ;
    rdfs:isDefinedBy dpv-owl: ;
    rdfs:subClassOf dpv-owl:EnforceSecurity ;
    sw:term_status "accepted"@en ;
    skos:definition "Prevention and Detection of Misuse or Abuse of services"@en ;
    skos:prefLabel "Misuse, Prevention and Detection"@en .

dpv-owl:MobilePlatformSecurity a rdfs:Class,
        owl:Class,
        dpv-owl:TechnicalMeasure ;
    dct:contributor "Harshvardhan J. Pandit" ;
    dct:created "2022-08-17"^^xsd:date ;
    dct:source [ a schema:WebPage ;
            schema:name "ENISA Reference Incident Classification Taxonomy 2018" ;
            schema:url "https://www.enisa.europa.eu/publications/reference-incident-classification-taxonomy/" ] ;
    rdfs:isDefinedBy dpv-owl: ;
    rdfs:subClassOf dpv-owl:SecurityMethod ;
    sw:term_status "accepted"@en ;
    skos:definition "Security implemented over a mobile platform"@en ;
    skos:prefLabel "Mobile Platform Security"@en .

dpv-owl:Modify a rdfs:Class,
        owl:Class,
        dpv-owl:Processing ;
    dct:contributor "Harshvardhan J. Pandit, Georg P. Krog" ;
    dct:created "2022-06-15"^^xsd:date ;
    rdfs:isDefinedBy dpv-owl: ;
    rdfs:subClassOf dpv-owl:Alter ;
    sw:term_status "accepted"@en ;
    skos:definition "to modify or change data"@en ;
    skos:prefLabel "Modify"@en .

dpv-owl:Monitor a rdfs:Class,
        owl:Class,
        dpv-owl:Processing ;
    dct:contributor "Harshvardhan J. Pandit, Georg P. Krog" ;
    dct:created "2022-06-15"^^xsd:date ;
    rdfs:isDefinedBy dpv-owl: ;
    rdfs:subClassOf dpv-owl:Consult ;
    sw:term_status "accepted"@en ;
    skos:definition "to monitor data for some criteria"@en ;
    skos:prefLabel "Monitor"@en .

dpv-owl:MonitoringPolicy a rdfs:Class,
        owl:Class,
        dpv-owl:OrganisationalMeasure ;
    dct:contributor "Harshvardhan J. Pandit" ;
    dct:created "2022-08-17"^^xsd:date ;
    dct:modified "2024-04-14"^^xsd:date ;
    dct:source [ a schema:WebPage ;
            schema:name "ENISA 5G Cybersecurity Standards" ;
            schema:url "https://www.enisa.europa.eu/publications/5g-cybersecurity-standards" ] ;
    rdfs:isDefinedBy dpv-owl: ;
    rdfs:subClassOf dpv-owl:Policy ;
    sw:term_status "accepted"@en ;
    skos:definition "Policy for monitoring (e.g. progress, performance)"@en ;
    skos:prefLabel "Monitoring Policy"@en .

dpv-owl:MonotonicCounterPseudonymisation a rdfs:Class,
        owl:Class,
        dpv-owl:TechnicalMeasure ;
    dct:contributor "Harshvardhan J. Pandit" ;
    dct:created "2022-08-17"^^xsd:date ;
    dct:modified "2022-10-13"^^xsd:date ;
    dct:source [ a schema:WebPage ;
            schema:name "ENISA Data Pseudonymisation: Advanced Techniques and Use Cases" ;
            schema:url "https://www.enisa.europa.eu/publications/data-pseudonymisation-advanced-techniques-and-use-cases" ] ;
    rdfs:isDefinedBy dpv-owl: ;
    rdfs:subClassOf dpv-owl:Pseudonymisation ;
    sw:term_status "accepted"@en ;
    skos:definition "A simple pseudonymisation method where identifiers are substituted by a number chosen by a monotonic counter"@en ;
    skos:prefLabel "Monotonic Counter Pseudonymisation"@en .

dpv-owl:Move a rdfs:Class,
        owl:Class,
        dpv-owl:Processing ;
    dct:created "2019-05-07"^^xsd:date ;
    dct:source [ a schema:WebPage ;
            schema:name "SPECIAL Project" ;
            schema:url "https://specialprivacy.ercim.eu/vocabs/processing" ] ;
    rdfs:isDefinedBy dpv-owl: ;
    rdfs:subClassOf dpv-owl:Transfer ;
    sw:term_status "accepted"@en ;
    skos:definition "to move data from one location to another including deleting the original copy"@en ;
    skos:prefLabel "Move"@en ;
    skos:related svpr:Move .

dpv-owl:MultiFactorAuthentication a rdfs:Class,
        owl:Class,
        dpv-owl:TechnicalMeasure ;
    dct:contributor "Harshvardhan J. Pandit" ;
    dct:created "2022-08-17"^^xsd:date ;
    dct:source [ a schema:WebPage ;
            schema:name "ENISA Reference Incident Classification Taxonomy 2018" ;
            schema:url "https://www.enisa.europa.eu/publications/reference-incident-classification-taxonomy/" ] ;
    rdfs:isDefinedBy dpv-owl: ;
    rdfs:subClassOf dpv-owl:AuthenticationProtocols ;
    sw:term_status "accepted"@en ;
    skos:definition "An authentication system that uses two or more methods to authenticate"@en ;
    skos:prefLabel "Multi-Factor Authentication (MFA)"@en .

dpv-owl:MultiNationalScale a rdfs:Class,
        owl:Class,
        dpv-owl:GeographicCoverage ;
    dct:contributor "Harshvardhan J. Pandit" ;
    dct:created "2022-06-15"^^xsd:date ;
    rdfs:isDefinedBy dpv-owl: ;
    rdfs:subClassOf dpv-owl:GeographicCoverage ;
    sw:term_status "accepted"@en ;
    skos:definition "Geographic coverage spanning multiple nations"@en ;
    skos:prefLabel "Multi National Scale"@en .

dpv-owl:NDA a rdfs:Class,
        owl:Class,
        dpv-owl:LegalMeasure ;
    dct:contributor "Axel Polleres, Rob Brennan, Harshvardhan J. Pandit, Mark Lizar" ;
    dct:created "2019-04-05"^^xsd:date ;
    rdfs:isDefinedBy dpv-owl: ;
    rdfs:subClassOf dpv-owl:LegalAgreement ;
    sw:term_status "accepted"@en ;
    skos:definition "Non-disclosure Agreements e.g. preserving confidentiality of information"@en ;
    skos:prefLabel "Non-Disclosure Agreement (NDA)"@en .

dpv-owl:NationalAuthority a rdfs:Class,
        owl:Class ;
    dct:contributor "Harshvardhan J. Pandit" ;
    dct:created "2022-02-02"^^xsd:date ;
    dct:source [ a schema:WebPage ;
            schema:name "ADMS controlled vocabulary" ;
            schema:url "http://purl.org/adms" ] ;
    rdfs:isDefinedBy dpv-owl: ;
    rdfs:subClassOf dpv-owl:Authority ;
    sw:term_status "accepted"@en ;
    skos:definition "An authority tasked with overseeing legal compliance for a nation"@en ;
    skos:prefLabel "National Authority"@en .

dpv-owl:NationalScale a rdfs:Class,
        owl:Class,
        dpv-owl:GeographicCoverage ;
    dct:contributor "Harshvardhan J. Pandit" ;
    dct:created "2022-06-15"^^xsd:date ;
    rdfs:isDefinedBy dpv-owl: ;
    rdfs:subClassOf dpv-owl:GeographicCoverage ;
    sw:term_status "accepted"@en ;
    skos:definition "Geographic coverage spanning a nation"@en ;
    skos:prefLabel "National Scale"@en .

dpv-owl:NaturalPerson a rdfs:Class,
        owl:Class ;
    dct:contributor "Harshvardhan J. Pandit" ;
    dct:created "2022-02-09"^^xsd:date ;
    rdfs:isDefinedBy dpv-owl: ;
    rdfs:subClassOf dpv-owl:Entity ;
    sw:term_status "accepted"@en ;
    skos:definition "A human"@en ;
    skos:prefLabel "Natural Person"@en .

dpv-owl:NearlyGlobalScale a rdfs:Class,
        owl:Class,
        dpv-owl:GeographicCoverage ;
    dct:contributor "Harshvardhan J. Pandit" ;
    dct:created "2022-06-15"^^xsd:date ;
    rdfs:isDefinedBy dpv-owl: ;
    rdfs:subClassOf dpv-owl:GeographicCoverage ;
    sw:term_status "accepted"@en ;
    skos:definition "Geographic coverage nearly spanning the entire globe"@en ;
    skos:prefLabel "Nearly Global Scale"@en .

dpv-owl:Necessity a rdfs:Class,
        owl:Class ;
    dct:contributor "Harshvardhan J. Pandit, Paul Ryan, Georg P. Krog, Julian Flake, Beatriz Esteves" ;
    dct:created "2022-02-12"^^xsd:date ;
    vann:example dex-owl:E0026,
        dex-owl:E0052 ;
    rdfs:isDefinedBy dpv-owl: ;
    rdfs:subClassOf dpv-owl:Context ;
    sw:term_status "accepted"@en ;
    skos:definition "An indication of 'necessity' within a context"@en ;
    skos:prefLabel "Necessity"@en ;
    skos:scopeNote "Necessity can be used to express need, essentiality, requirement, or compulsion."@en .

dpv-owl:NetworkProxyRouting a rdfs:Class,
        owl:Class,
        dpv-owl:TechnicalMeasure ;
    dct:contributor "Harshvardhan J. Pandit" ;
    dct:created "2022-08-17"^^xsd:date ;
    dct:source [ a schema:WebPage ;
            schema:name "ENISA Data Protection Engineering" ;
            schema:url "https://www.enisa.europa.eu/publications/data-protection-engineering" ] ;
    rdfs:isDefinedBy dpv-owl: ;
    rdfs:subClassOf dpv-owl:SecurityMethod ;
    sw:term_status "accepted"@en ;
    skos:definition "Use of network routing using proxy"@en ;
    skos:prefLabel "Network Proxy Routing"@en .

dpv-owl:NetworkSecurityProtocols a rdfs:Class,
        owl:Class,
        dpv-owl:TechnicalMeasure ;
    dct:contributor "Harshvardhan J. Pandit" ;
    dct:created "2022-08-17"^^xsd:date ;
    dct:source [ a schema:WebPage ;
            schema:name "ENISA Reference Incident Classification Taxonomy 2018" ;
            schema:url "https://www.enisa.europa.eu/publications/reference-incident-classification-taxonomy/" ] ;
    rdfs:isDefinedBy dpv-owl: ;
    rdfs:subClassOf dpv-owl:SecurityMethod ;
    sw:term_status "accepted"@en ;
    skos:definition "Security implemented at or over networks protocols"@en ;
    skos:prefLabel "Network Security Protocols"@en .

dpv-owl:NonCitizen a rdfs:Class,
        owl:Class,
        dpv-owl:DataSubject ;
    dct:contributor "Harshvardhan J. Pandit, Georg P. Krog, Julian Flake, Paul Ryan, Beatriz Esteves" ;
    dct:created "2022-04-06"^^xsd:date ;
    rdfs:isDefinedBy dpv-owl: ;
    rdfs:subClassOf dpv-owl:DataSubject ;
    sw:term_status "accepted"@en ;
    skos:definition "Data subjects that are not citizens (for a jurisdiction)"@en ;
    skos:prefLabel "Non-Citizen"@en .

dpv-owl:NonCommercialPurpose a rdfs:Class,
        owl:Class,
        dpv-owl:Purpose ;
    dct:contributor "Beatriz Esteves, Harshvardhan J. Pandit" ;
    dct:created "2024-02-14"^^xsd:date ;
    dct:source "DGA 4.4"@en ;
    rdfs:isDefinedBy dpv-owl: ;
    rdfs:subClassOf dpv-owl:Purpose ;
    sw:term_status "accepted"@en ;
    skos:definition "Purposes associated with processing activities performed in a non-commercial setting or without intention to commercialise"@en ;
    skos:prefLabel "Non-commercial Purpose"@en .

dpv-owl:NonCommercialResearch a rdfs:Class,
        owl:Class,
        dpv-owl:Purpose ;
    dct:contributor "Harshvardhan J. Pandit, Javier Fernández, Axel Polleres, Elmar Kiesling, Fajar Ekaputra, Simon Steyskal" ;
    dct:created "2019-04-05"^^xsd:date ;
    dct:modified "2024-04-14"^^xsd:date ;
    rdfs:isDefinedBy dpv-owl: ;
    rdfs:subClassOf dpv-owl:NonCommercialPurpose,
        dpv-owl:ResearchAndDevelopment ;
    sw:term_status "accepted"@en ;
    skos:definition "Purposes associated with conducting research in a non-commercial setting e.g. for a non-profit-organisation (NGO)"@en ;
    skos:prefLabel "Non-Commercial Research"@en .

dpv-owl:NonCompliant a rdfs:Class,
        owl:Class,
        dpv-owl:ComplianceStatus ;
    dct:contributor "Harshvardhan J. Pandit" ;
    dct:created "2022-05-18"^^xsd:date ;
    dct:modified "2022-09-07"^^xsd:date ;
    rdfs:isDefinedBy dpv-owl: ;
    rdfs:subClassOf dpv-owl:ComplianceStatus ;
    sw:term_status "accepted"@en ;
    skos:definition "State of non-compliance where objectives have not been met, but have not been violated"@en ;
    skos:prefLabel "Non Compliant"@en ;
    skos:scopeNote "Changed from not compliant for consistency in commonly used terms"@en .

dpv-owl:NonConformant a rdfs:Class,
        owl:Class,
        dpv-owl:ConformanceStatus ;
    dct:contributor "Harshvardhan J. Pandit" ;
    dct:created "2022-10-22"^^xsd:date ;
    rdfs:isDefinedBy dpv-owl: ;
    rdfs:subClassOf dpv-owl:ConformanceStatus ;
    sw:term_status "accepted"@en ;
    skos:definition "State of being non-conformant"@en ;
    skos:prefLabel "NonConformant"@en .

dpv-owl:NonGovernmentalOrganisation a rdfs:Class,
        owl:Class ;
    dct:contributor "Harshvardhan J. Pandit" ;
    dct:created "2022-02-02"^^xsd:date ;
    dct:modified "2020-10-05"^^xsd:date ;
    dct:source [ a schema:WebPage ;
            schema:name "ADMS controlled vocabulary" ;
            schema:url "http://purl.org/adms" ] ;
    rdfs:isDefinedBy dpv-owl: ;
    rdfs:subClassOf dpv-owl:Organisation ;
    sw:term_status "accepted"@en ;
    skos:definition "An organisation not part of or independent from the government"@en ;
    skos:prefLabel "Non-Governmental Organisation"@en .

dpv-owl:NonPersonalData a rdfs:Class,
        owl:Class ;
    dct:contributor "Harshvardhan J. Pandit" ;
    dct:created "2022-01-19"^^xsd:date ;
    rdfs:isDefinedBy dpv-owl: ;
    rdfs:subClassOf dpv-owl:Data ;
    sw:term_status "accepted"@en ;
    skos:definition "Data that is not Personal Data"@en ;
    skos:prefLabel "Non-Personal Data"@en ;
    skos:scopeNote "The term NonPersonalData is provided to distinguish between PersonalData and other data, e.g. for indicating which data is regulated by privacy laws. To specify personal data that has been anonymised, the concept AnonymisedData should be used as the anonymisation process has a risk of not being fully effective and such anonymous data may be found to be personal data depending on circumstances."@en .

dpv-owl:NonPersonalDataProcess a rdfs:Class,
        owl:Class ;
    dct:contributor "Harshvardhan J. Pandit" ;
    dct:created "2024-05-09"^^xsd:date ;
    rdfs:isDefinedBy dpv-owl: ;
    rdfs:subClassOf dpv-owl:Process ;
    sw:term_status "accepted"@en ;
    skos:definition "An action, activity, or method involving non-personal data, and asserting that no personal data is involved"@en ;
    skos:prefLabel "Non-Personal Data Process"@en ;
    skos:scopeNote "Use of personal data within NonPersonalDataProcess should be considered a violation of the explicit constraint that no personal data is involved."@en .

dpv-owl:NonProfitOrganisation a rdfs:Class,
        owl:Class ;
    dct:contributor "Harshvardhan J. Pandit" ;
    dct:created "2022-02-02"^^xsd:date ;
    dct:modified "2020-10-05"^^xsd:date ;
    dct:source [ a schema:WebPage ;
            schema:name "ADMS controlled vocabulary" ;
            schema:url "http://purl.org/adms" ] ;
    rdfs:isDefinedBy dpv-owl: ;
    rdfs:subClassOf dpv-owl:Organisation ;
    sw:term_status "accepted"@en ;
    skos:definition "An organisation that does not aim to achieve profit as its primary goal"@en ;
    skos:prefLabel "Non-Profit Organisation"@en .

dpv-owl:NonPublicDataSource a rdfs:Class,
        owl:Class,
        dpv-owl:DataSource ;
    dct:contributor "Georg P. Krog, Harshvardhan J. Pandit, Beatriz Esteves, Paul Ryan, Julian Flake" ;
    dct:created "2022-01-26"^^xsd:date ;
    rdfs:isDefinedBy dpv-owl: ;
    rdfs:subClassOf dpv-owl:DataSource ;
    sw:term_status "accepted"@en ;
    skos:definition "A source of data that is not publicly accessible or available"@en ;
    skos:prefLabel "Non-Public Data Source"@en .

dpv-owl:NotApplicable a rdfs:Class,
        owl:Class,
        dpv-owl:Applicability ;
    dct:contributor "Harshvardhan J. Pandit" ;
    dct:created "2023-08-24"^^xsd:date ;
    rdfs:isDefinedBy dpv-owl: ;
    rdfs:subClassOf dpv-owl:Applicability ;
    sw:term_status "accepted"@en ;
    skos:definition "Concept indicating the information or context is not applicable"@en ;
    skos:prefLabel "Not Applicable"@en ;
    skos:scopeNote "This relates to a 'Stop' state as distinct from a 'Halt' state. It makes no comments on whether the Activity can be resumed or continued towards completion."@en .

dpv-owl:NotAutomated a rdfs:Class,
        owl:Class,
        dpv-owl:AutomationLevel ;
    dct:contributor "Harshvardhan J. Pandit, Delaram Golpayegani" ;
    dct:created "2023-12-10"^^xsd:date ;
    dct:modified "2024-04-20"^^xsd:date ;
    dct:source [ a schema:WebPage ;
            schema:name "ISO/IEC 22989:2022 Artificial intelligence concepts and terminology" ;
            schema:url "https://www.iso.org/standard/74296.html" ] ;
    rdfs:isDefinedBy dpv-owl: ;
    rdfs:subClassOf dpv-owl:AutomationLevel ;
    sw:term_status "accepted"@en ;
    skos:definition "Level of automation corresponding to Level 0 in ISO/IEC 22989:2022 where there is no automation in the system"@en ;
    skos:prefLabel "Not Automated"@en ;
    skos:scopeNote "Human Involvement is necessary here as there is no automation"@en .

dpv-owl:NotAvailable a rdfs:Class,
        owl:Class,
        dpv-owl:Applicability ;
    dct:contributor "Harshvardhan J. Pandit" ;
    dct:created "2023-08-24"^^xsd:date ;
    rdfs:isDefinedBy dpv-owl: ;
    rdfs:subClassOf dpv-owl:Applicability ;
    sw:term_status "accepted"@en ;
    skos:definition "Concept indicating the information or context is applicable but information is not yet available"@en ;
    skos:prefLabel "Not Available"@en ;
    skos:scopeNote "This concept is useful when describing situations where information is required but is not available (yet). For example, if in a form a field asks about whether a process X was completed, and it is correct to interpret that process X is applicable and must be completed, but the information is not yet available as to whether this was done - then NotAvailable is useful to represent this."@en .

dpv-owl:NotInvolved a rdfs:Class,
        owl:Class,
        dpv-owl:InvolvementStatus ;
    dct:contributor "Harshvardhan J. Pandit, Delaram Golpayegani, Georg P. Krog, Paul Ryan" ;
    dct:created "2024-05-10"^^xsd:date ;
    rdfs:isDefinedBy dpv-owl: ;
    rdfs:subClassOf dpv-owl:InvolvementStatus ;
    sw:term_status "accepted"@en ;
    skos:definition "Status indicating the specified context is 'not' involved"@en ;
    skos:prefLabel "Not Involved"@en .

dpv-owl:NotRequired a rdfs:Class,
        owl:Class,
        dpv-owl:Necessity ;
    dct:contributor "Harshvardhan J. Pandit, Paul Ryan, Georg P. Krog, Julian Flake, Beatriz Esteves" ;
    dct:created "2022-02-15"^^xsd:date ;
    rdfs:isDefinedBy dpv-owl: ;
    rdfs:subClassOf dpv-owl:Necessity ;
    sw:term_status "accepted"@en ;
    skos:definition "Indication of neither being required nor optional i.e. not relevant or needed"@en ;
    skos:prefLabel "Not Required"@en .

dpv-owl:Notice a rdfs:Class,
        owl:Class,
        dpv-owl:OrganisationalMeasure ;
    dct:contributor "Paul Ryan, David Hickey, Georg P. Krog, Harshvardhan J. Pandit" ;
    dct:created "2021-09-08"^^xsd:date ;
    vann:example dex-owl:E0017 ;
    rdfs:isDefinedBy dpv-owl: ;
    rdfs:subClassOf dpv-owl:OrganisationalMeasure ;
    sw:term_status "accepted"@en ;
    skos:definition "A notice is an artefact for providing information, choices, or controls"@en ;
    skos:prefLabel "Notice"@en ;
    skos:scopeNote "Notice refers to the information whereas Notification refers to the provision of that notice. In several cases, they are used interchangeably - for example Privacy Notice as a measure or control refers to both the information as well as the act of making it available. For 'active' contexts where this distinction is important, e.g. data breach notifications, see Notification concept."@en .

dpv-owl:Notification a rdfs:Class,
        owl:Class,
        dpv-owl:OrganisationalMeasure ;
    dct:contributor "Harshvardhan J. Pandit" ;
    dct:created "2024-04-14"^^xsd:date ;
    rdfs:isDefinedBy dpv-owl: ;
    rdfs:subClassOf dpv-owl:OrganisationalMeasure ;
    sw:term_status "accepted"@en ;
    skos:definition "Notification represents the provision of a notice i.e. notifying"@en ;
    skos:prefLabel "Notification"@en ;
    skos:scopeNote "Notice refers to the information whereas Notification refers to the provision of that notice. The distinction is important as there are specific obligations associated with notice and notifications. For example, a data breach notice refers to the information about the breach intended to be provided to another entity, whereas notification refers to the act of providing the entity with the notice"@en .

dpv-owl:NotificationCompleted a rdfs:Class,
        owl:Class,
        dpv-owl:NotificationStatus ;
    dct:contributor "Harshvardhan J. Pandit" ;
    dct:created "2024-05-19"^^xsd:date ;
    rdfs:isDefinedBy dpv-owl: ;
    rdfs:subClassOf dpv-owl:NotificationStatus ;
    sw:term_status "accepted"@en ;
    skos:definition "Status indicating notification(s) are completed"@en ;
    skos:prefLabel "Notification Completed"@en .

dpv-owl:NotificationFailed a rdfs:Class,
        owl:Class,
        dpv-owl:NotificationStatus ;
    dct:contributor "Harshvardhan J. Pandit" ;
    dct:created "2024-05-19"^^xsd:date ;
    rdfs:isDefinedBy dpv-owl: ;
    rdfs:subClassOf dpv-owl:NotificationStatus ;
    sw:term_status "accepted"@en ;
    skos:definition "Status indicating notification(s) could not be completed due to a failure"@en ;
    skos:prefLabel "Notification Failed"@en .

dpv-owl:NotificationNotNeeded a rdfs:Class,
        owl:Class,
        dpv-owl:NotificationStatus ;
    dct:contributor "Harshvardhan J. Pandit" ;
    dct:created "2024-05-19"^^xsd:date ;
    rdfs:isDefinedBy dpv-owl: ;
    rdfs:subClassOf dpv-owl:NotificationStatus ;
    sw:term_status "accepted"@en ;
    skos:definition "Status indicating notification(s) are not needed"@en ;
    skos:prefLabel "Notification Not Needed"@en .

dpv-owl:NotificationOngoing a rdfs:Class,
        owl:Class,
        dpv-owl:NotificationStatus ;
    dct:contributor "Harshvardhan J. Pandit" ;
    dct:created "2024-05-19"^^xsd:date ;
    rdfs:isDefinedBy dpv-owl: ;
    rdfs:subClassOf dpv-owl:NotificationStatus ;
    sw:term_status "accepted"@en ;
    skos:definition "Status indicating notification(s) are ongoing"@en ;
    skos:prefLabel "Notification Ongoing"@en .

dpv-owl:NotificationPlanned a rdfs:Class,
        owl:Class,
        dpv-owl:NotificationStatus ;
    dct:contributor "Harshvardhan J. Pandit" ;
    dct:created "2024-05-19"^^xsd:date ;
    rdfs:isDefinedBy dpv-owl: ;
    rdfs:subClassOf dpv-owl:NotificationStatus ;
    sw:term_status "accepted"@en ;
    skos:definition "Status indicating notification(s) are planned"@en ;
    skos:prefLabel "Notification Planned"@en .

dpv-owl:NotificationStatus a rdfs:Class,
        owl:Class ;
    dct:contributor "Harshvardhan J. Pandit" ;
    dct:created "2024-05-19"^^xsd:date ;
    rdfs:isDefinedBy dpv-owl: ;
    rdfs:subClassOf dpv-owl:Status ;
    sw:term_status "accepted"@en ;
    skos:definition "Status indicating whether notification(s) are planned, completed, or failed"@en ;
    skos:prefLabel "Notification Status"@en .

dpv-owl:ObjectingToProcess a rdfs:Class,
        owl:Class,
        dpv-owl:EntityPermissiveInvolvement ;
    dct:contributor "Harshvardhan J. Pandit, Delaram Golpayegani, Steve Hickman" ;
    dct:created "2024-05-11"^^xsd:date ;
    rdfs:isDefinedBy dpv-owl: ;
    rdfs:subClassOf dpv-owl:EntityPermissiveInvolvement ;
    sw:term_status "accepted"@en ;
    skos:definition "Involvement where entity can object to process of specified context"@en ;
    skos:prefLabel "Objecting to Process"@en .

dpv-owl:Obligation a rdfs:Class,
        owl:Class,
        dpv-owl:Rule ;
    dct:contributor "Harshvardhan J. Pandit, Georg P. Krog, Beatriz Esteves, Paul Ryan" ;
    dct:created "2022-10-19"^^xsd:date ;
    rdfs:isDefinedBy dpv-owl: ;
    rdfs:subClassOf dpv-owl:Rule ;
    sw:term_status "accepted"@en ;
    skos:definition "A rule describing an obligation for performing an activity"@en ;
    skos:prefLabel "Obligation"@en .

dpv-owl:Observe a rdfs:Class,
        owl:Class,
        dpv-owl:Processing ;
    dct:contributor "Harshvardhan J. Pandit, Georg P. Krog" ;
    dct:created "2022-06-15"^^xsd:date ;
    rdfs:isDefinedBy dpv-owl: ;
    rdfs:subClassOf dpv-owl:Obtain ;
    sw:term_status "accepted"@en ;
    skos:definition "to obtain data through observation"@en ;
    skos:prefLabel "Observe"@en .

dpv-owl:ObservedData a rdfs:Class,
        owl:Class ;
    dct:created "2023-12-10"^^xsd:date ;
    rdfs:isDefinedBy dpv-owl: ;
    rdfs:subClassOf dpv-owl:CollectedData ;
    sw:term_status "accepted"@en ;
    skos:definition "Data that has been obtained through observations of a source"@en ;
    skos:prefLabel "Observed Data"@en .

dpv-owl:ObservedPersonalData a rdfs:Class,
        owl:Class ;
    dct:contributor "Georg P. Krog" ;
    dct:created "2022-08-24"^^xsd:date ;
    dct:modified "2023-12-10"^^xsd:date ;
    rdfs:isDefinedBy dpv-owl: ;
    rdfs:subClassOf dpv-owl:CollectedPersonalData,
        dpv-owl:ObservedData ;
    sw:term_status "accepted"@en ;
    skos:definition "Personal Data that has been collected through observation of the Data Subject(s)"@en ;
    skos:prefLabel "Observed Personal Data"@en .

dpv-owl:Obtain a rdfs:Class,
        owl:Class,
        dpv-owl:Processing ;
    dct:created "2019-05-07"^^xsd:date ;
    dct:source [ a schema:WebPage ;
            schema:name "GDPR Art.4-2" ;
            schema:url "https://eur-lex.europa.eu/eli/reg/2016/679/art_4/par_2/oj" ] ;
    rdfs:isDefinedBy dpv-owl: ;
    rdfs:subClassOf dpv-owl:Processing ;
    sw:term_status "accepted"@en ;
    skos:definition "to solicit or gather data from someone"@en ;
    skos:prefLabel "Obtain"@en .

dpv-owl:ObtainConsent a rdfs:Class,
        owl:Class ;
    dct:created "2024-05-11"^^xsd:date ;
    rdfs:isDefinedBy dpv-owl: ;
    rdfs:subClassOf dpv-owl:ConsentControl ;
    sw:term_status "accepted"@en ;
    skos:definition "Control for obtaining consent"@en ;
    skos:prefLabel "Obtain Consent"@en ;
    skos:scopeNote "Indicates how the controller or entity can obtain consent e.g. used with dpv:isExercisedAt"@en .

dpv-owl:OfficialAuthorityOfController a rdfs:Class,
        owl:Class,
        dpv-owl:LegalBasis ;
    dct:contributor "Georg P. Krog, Harshvardhan J. Pandit, Paul Ryan" ;
    dct:created "2021-05-05"^^xsd:date ;
    rdfs:isDefinedBy dpv-owl: ;
    rdfs:subClassOf dpv-owl:LegalBasis ;
    sw:term_status "accepted"@en ;
    skos:definition "Activities are necessary or authorised through the official authority granted to or vested in the Data Controller"@en ;
    skos:prefLabel "Official Authority of Controller"@en .

dpv-owl:OftenFrequency a rdfs:Class,
        owl:Class,
        dpv-owl:Frequency ;
    dct:contributor "Harshvardhan J. Pandit" ;
    dct:created "2022-06-15"^^xsd:date ;
    dct:modified "2020-10-05"^^xsd:date ;
    rdfs:isDefinedBy dpv-owl: ;
    rdfs:subClassOf dpv-owl:Frequency ;
    sw:term_status "accepted"@en ;
    skos:definition "Frequency where occurrences are often or frequent, but not continuous"@en ;
    skos:prefLabel "Often Frequency"@en .

dpv-owl:OperatingSystemSecurity a rdfs:Class,
        owl:Class,
        dpv-owl:TechnicalMeasure ;
    dct:contributor "Harshvardhan J. Pandit" ;
    dct:created "2022-08-17"^^xsd:date ;
    dct:source [ a schema:WebPage ;
            schema:name "ENISA Reference Incident Classification Taxonomy 2018" ;
            schema:url "https://www.enisa.europa.eu/publications/reference-incident-classification-taxonomy/" ] ;
    rdfs:isDefinedBy dpv-owl: ;
    rdfs:subClassOf dpv-owl:SecurityMethod ;
    sw:term_status "accepted"@en ;
    skos:definition "Security implemented at or through operating systems"@en ;
    skos:prefLabel "Operating System Security"@en .

dpv-owl:OptimisationForConsumer a rdfs:Class,
        owl:Class,
        dpv-owl:Purpose ;
    dct:contributor "Harshvardhan J. Pandit, Javier Fernández, Axel Polleres, Elmar Kiesling, Fajar Ekaputra, Simon Steyskal" ;
    dct:created "2019-04-05"^^xsd:date ;
    rdfs:isDefinedBy dpv-owl: ;
    rdfs:subClassOf dpv-owl:ServiceOptimisation ;
    sw:term_status "accepted"@en ;
    skos:definition "Purposes associated with optimisation of activities and services for consumer or user"@en ;
    skos:prefLabel "Optimisation for Consumer"@en ;
    skos:related svpu:Custom ;
    skos:scopeNote "The term optimisation here refers to the efficiency of the service in terms of technical provision (or similar means) with benefits for everybody. Personalisation implies making changes that benefit the current user or persona."@en .

dpv-owl:OptimisationForController a rdfs:Class,
        owl:Class,
        dpv-owl:Purpose ;
    dct:contributor "Harshvardhan J. Pandit, Javier Fernández, Axel Polleres, Elmar Kiesling, Fajar Ekaputra, Simon Steyskal" ;
    dct:created "2019-04-05"^^xsd:date ;
    rdfs:isDefinedBy dpv-owl: ;
    rdfs:subClassOf dpv-owl:ServiceOptimisation ;
    sw:term_status "accepted"@en ;
    skos:definition "Purposes associated with optimisation of activities and services for provider or controller"@en ;
    skos:prefLabel "Optimisation for Controller"@en .

dpv-owl:OptimiseUserInterface a rdfs:Class,
        owl:Class,
        dpv-owl:Purpose ;
    dct:contributor "Harshvardhan J. Pandit, Javier Fernández, Axel Polleres, Elmar Kiesling, Fajar Ekaputra, Simon Steyskal" ;
    dct:created "2019-04-05"^^xsd:date ;
    rdfs:isDefinedBy dpv-owl: ;
    rdfs:subClassOf dpv-owl:OptimisationForConsumer ;
    sw:term_status "accepted"@en ;
    skos:definition "Purposes associated with optimisation of interfaces presented to the user"@en ;
    skos:prefLabel "Optimise User Interface"@en .

dpv-owl:OptingInToProcess a rdfs:Class,
        owl:Class,
        dpv-owl:EntityPermissiveInvolvement ;
    dct:contributor "Harshvardhan J. Pandit, Delaram Golpayegani, Steve Hickman" ;
    dct:created "2024-05-11"^^xsd:date ;
    rdfs:isDefinedBy dpv-owl: ;
    rdfs:subClassOf dpv-owl:EntityPermissiveInvolvement ;
    sw:term_status "accepted"@en ;
    skos:definition "Involvement where entity can opt-in to specified context"@en ;
    skos:prefLabel "Opting in to Process"@en .

dpv-owl:OptingOutFromProcess a rdfs:Class,
        owl:Class,
        dpv-owl:EntityPermissiveInvolvement ;
    dct:contributor "Harshvardhan J. Pandit, Delaram Golpayegani, Steve Hickman" ;
    dct:created "2024-05-11"^^xsd:date ;
    rdfs:isDefinedBy dpv-owl: ;
    rdfs:subClassOf dpv-owl:EntityPermissiveInvolvement ;
    sw:term_status "accepted"@en ;
    skos:definition "Involvement where entity can opt-out from specified context"@en ;
    skos:prefLabel "Opting out of Process"@en .

dpv-owl:Optional a rdfs:Class,
        owl:Class,
        dpv-owl:Necessity ;
    dct:contributor "Harshvardhan J. Pandit, Paul Ryan, Georg P. Krog, Julian Flake, Beatriz Esteves" ;
    dct:created "2022-02-14"^^xsd:date ;
    rdfs:isDefinedBy dpv-owl: ;
    rdfs:subClassOf dpv-owl:Necessity ;
    sw:term_status "accepted"@en ;
    skos:definition "Indication of 'optional' or 'voluntary'"@en ;
    skos:prefLabel "Optional"@en .

dpv-owl:Organisation a rdfs:Class,
        owl:Class ;
    dct:contributor "Harshvardhan J. Pandit" ;
    dct:created "2022-02-02"^^xsd:date ;
    rdfs:isDefinedBy dpv-owl: ;
    rdfs:subClassOf dpv-owl:LegalEntity ;
    sw:term_status "accepted"@en ;
    skos:definition "A general term reflecting a company or a business or a group acting as a unit"@en ;
    skos:prefLabel "Organisation"@en .

dpv-owl:OrganisationComplianceManagement a rdfs:Class,
        owl:Class,
        dpv-owl:Purpose ;
    dct:contributor "Paul Ryan, Georg P. Krog, David Hickey, Harshvardhan J. Pandit" ;
    dct:created "2021-09-01"^^xsd:date ;
    rdfs:isDefinedBy dpv-owl: ;
    rdfs:subClassOf dpv-owl:OrganisationGovernance ;
    sw:term_status "accepted"@en ;
    skos:definition "Purposes associated with managing compliance for organisation in relation to internal policies"@en ;
    skos:prefLabel "Organisation Compliance Management"@en ;
    skos:scopeNote "Note that this concept relates to internal organisational compliance. The concept LegalCompliance should be used for external legal or regulatory compliance."@en .

dpv-owl:OrganisationGovernance a rdfs:Class,
        owl:Class,
        dpv-owl:Purpose ;
    dct:contributor "Paul Ryan, Georg P. Krog, David Hickey, Harshvardhan J. Pandit" ;
    dct:created "2021-09-01"^^xsd:date ;
    dct:source [ a schema:WebPage ;
            schema:name "Belgian DPA ROPA Template" ;
            schema:url "https://www.privacycommission.be/nl/model-voor-een-register-van-de-verwerkingsactiviteiten" ] ;
    rdfs:isDefinedBy dpv-owl: ;
    rdfs:subClassOf dpv-owl:Purpose ;
    sw:term_status "accepted"@en ;
    skos:definition "Purposes associated with conducting activities and functions for governance of an organisation"@en ;
    skos:prefLabel "Organisation Governance"@en .

dpv-owl:OrganisationRiskManagement a rdfs:Class,
        owl:Class,
        dpv-owl:Purpose ;
    dct:contributor "Paul Ryan, Georg P. Krog, David Hickey, Harshvardhan J. Pandit" ;
    dct:created "2021-09-01"^^xsd:date ;
    rdfs:isDefinedBy dpv-owl: ;
    rdfs:subClassOf dpv-owl:OrganisationGovernance ;
    sw:term_status "accepted"@en ;
    skos:definition "Purposes associated with managing risk for organisation's activities"@en ;
    skos:prefLabel "Organisation Risk Management"@en .

dpv-owl:OrganisationalMeasure a rdfs:Class,
        owl:Class ;
    dct:contributor "Axel Polleres, Rob Brennan, Harshvardhan J. Pandit, Mark Lizar" ;
    dct:created "2019-04-05"^^xsd:date ;
    dct:modified "2023-12-10"^^xsd:date ;
    vann:example dex-owl:E0021 ;
    rdfs:isDefinedBy dpv-owl: ;
    rdfs:subClassOf dpv-owl:TechnicalOrganisationalMeasure ;
    sw:term_status "accepted"@en ;
    skos:definition "Organisational measures used to safeguard and ensure good practices in connection with data and technologies"@en ;
    skos:prefLabel "Organisational Measure"@en .

dpv-owl:OrganisationalUnit a rdfs:Class,
        owl:Class ;
    dct:contributor "Harshvardhan J. Pandit, Paul Ryan" ;
    dct:created "2022-03-23"^^xsd:date ;
    vann:example dex-owl:E0037 ;
    rdfs:isDefinedBy dpv-owl: ;
    rdfs:subClassOf dpv-owl:Entity ;
    sw:term_status "accepted"@en ;
    skos:definition "Entity within an organisation that does not constitute as a separate legal entity"@en ;
    skos:prefLabel "Organisational Unit"@en .

dpv-owl:Organise a rdfs:Class,
        owl:Class,
        dpv-owl:Processing ;
    dct:created "2019-05-07"^^xsd:date ;
    dct:source [ a schema:WebPage ;
            schema:name "GDPR Art.4-2" ;
            schema:url "https://eur-lex.europa.eu/eli/reg/2016/679/art_4/par_2/oj" ] ;
    rdfs:isDefinedBy dpv-owl: ;
    rdfs:subClassOf dpv-owl:Processing ;
    sw:term_status "accepted"@en ;
    skos:definition "to organize data for arranging or classifying"@en ;
    skos:prefLabel "Organise"@en .

dpv-owl:PIA a rdfs:Class,
        owl:Class,
        dpv-owl:OrganisationalMeasure ;
    dct:contributor "Georg P. Krog, Harshvardhan J. Pandit, Paul Ryan" ;
    dct:created "2020-11-04"^^xsd:date ;
    rdfs:isDefinedBy dpv-owl: ;
    rdfs:subClassOf dpv-owl:ImpactAssessment ;
    sw:term_status "accepted"@en ;
    skos:definition "Impact assessment regarding privacy risks"@en ;
    skos:prefLabel "Privacy Impact Assessment (PIA)"@en .

dpv-owl:ParentLegalEntity a rdfs:Class,
        owl:Class ;
    dct:contributor "Harshvardhan J. Pandit, Georg P. Krog" ;
    dct:created "2024-04-14"^^xsd:date ;
    rdfs:isDefinedBy dpv-owl: ;
    rdfs:subClassOf dpv-owl:Organisation ;
    sw:term_status "accepted"@en ;
    skos:definition "A legal entity that has one or more subsidiary entities operating under it"@en ;
    skos:prefLabel "Parent Legal Entity"@en .

dpv-owl:ParentOfDataSubject a rdfs:Class,
        owl:Class,
        dpv-owl:DataSubject ;
    dct:contributor "Georg P. Krog" ;
    dct:created "2022-08-03"^^xsd:date ;
    rdfs:isDefinedBy dpv-owl: ;
    rdfs:subClassOf dpv-owl:DataSubject ;
    sw:term_status "accepted"@en ;
    skos:definition "Parent(s) of data subjects such as children"@en ;
    skos:prefLabel "Parent(s) of Data Subject"@en .

dpv-owl:PartialAutomation a rdfs:Class,
        owl:Class,
        dpv-owl:AutomationLevel ;
    dct:contributor "Harshvardhan J. Pandit, Delaram Golpayegani" ;
    dct:created "2023-12-10"^^xsd:date ;
    dct:modified "2024-04-20"^^xsd:date ;
    dct:source [ a schema:WebPage ;
            schema:name "ISO/IEC 22989:2022 Artificial intelligence concepts and terminology" ;
            schema:url "https://www.iso.org/standard/74296.html" ] ;
    rdfs:isDefinedBy dpv-owl: ;
    rdfs:subClassOf dpv-owl:AutomationLevel ;
    sw:term_status "accepted"@en ;
    skos:definition "Level of automation corresponding to Level 2 in ISO/IEC 22989:2022 where the automation is present in multiple parts of the system or in a manner that does not require the human to control/use these parts while still retaining control over the system"@en ;
    skos:prefLabel "Partial Automation"@en ;
    skos:scopeNote "Human Involvement is implied here, specifically the ability to Control operations, but also possibly for intervention, oversight, and verification"@en .

dpv-owl:PartiallyCompliant a rdfs:Class,
        owl:Class,
        dpv-owl:ComplianceStatus ;
    dct:contributor "Harshvardhan J. Pandit" ;
    dct:created "2022-05-18"^^xsd:date ;
    rdfs:isDefinedBy dpv-owl: ;
    rdfs:subClassOf dpv-owl:ComplianceStatus ;
    sw:term_status "accepted"@en ;
    skos:definition "State of partially being compliant i.e. only some objectives have been met, and others have not been in violation"@en ;
    skos:prefLabel "Partially Compliant"@en .

dpv-owl:Participant a rdfs:Class,
        owl:Class,
        dpv-owl:DataSubject ;
    dct:contributor "Harshvardhan J. Pandit, Georg P. Krog, Julian Flake, Paul Ryan, Beatriz Esteves" ;
    dct:created "2022-04-06"^^xsd:date ;
    rdfs:isDefinedBy dpv-owl: ;
    rdfs:subClassOf dpv-owl:DataSubject ;
    sw:term_status "accepted"@en ;
    skos:definition "Data subjects that participate in some context such as volunteers in a function"@en ;
    skos:prefLabel "Participant"@en .

dpv-owl:PassiveRight a rdfs:Class,
        owl:Class,
        dpv-owl:Right ;
    dct:contributor "Harshvardhan J. Pandit, Beatriz Esteves, Georg P. Krog, Paul Ryan" ;
    dct:created "2022-10-22"^^xsd:date ;
    rdfs:isDefinedBy dpv-owl: ;
    rdfs:subClassOf dpv-owl:Right ;
    sw:term_status "accepted"@en ;
    skos:definition "The right(s) applicable, provided, or expected that are always (passively) applicable"@en ;
    skos:prefLabel "Passive Right"@en ;
    skos:scopeNote "Passive rights do not require the entity to request or exercise them. They are considered to be always applicable. For example, the Right to Privacy (in EU) does not require an exercise for it to be fulfilled."@en .

dpv-owl:PassivelyInvolved a rdfs:Class,
        owl:Class,
        dpv-owl:InvolvementStatus ;
    dct:contributor "Harshvardhan J. Pandit, Delaram Golpayegani, Georg P. Krog, Paul Ryan" ;
    dct:created "2024-05-10"^^xsd:date ;
    rdfs:isDefinedBy dpv-owl: ;
    rdfs:subClassOf dpv-owl:InvolvementStatus ;
    sw:term_status "accepted"@en ;
    skos:definition "Status indicating the specified context is 'passively' involved"@en ;
    skos:prefLabel "Passively Involved"@en ;
    skos:scopeNote "An example of passive involvement is a person being monitored by a CCTV"@en .

dpv-owl:PasswordAuthentication a rdfs:Class,
        owl:Class,
        dpv-owl:TechnicalMeasure ;
    dct:contributor "Harshvardhan J. Pandit" ;
    dct:created "2022-08-17"^^xsd:date ;
    dct:source [ a schema:WebPage ;
            schema:name "ENISA Reference Incident Classification Taxonomy 2018" ;
            schema:url "https://www.enisa.europa.eu/publications/reference-incident-classification-taxonomy/" ] ;
    rdfs:isDefinedBy dpv-owl: ;
    rdfs:subClassOf dpv-owl:AuthenticationProtocols ;
    sw:term_status "accepted"@en ;
    skos:definition "Use of passwords to perform authentication"@en ;
    skos:prefLabel "Password Authentication"@en .

dpv-owl:Patient a rdfs:Class,
        owl:Class,
        dpv-owl:DataSubject ;
    dct:contributor "Harshvardhan J. Pandit, Georg P. Krog, Julian Flake, Paul Ryan, Beatriz Esteves" ;
    dct:created "2022-04-06"^^xsd:date ;
    rdfs:isDefinedBy dpv-owl: ;
    rdfs:subClassOf dpv-owl:DataSubject ;
    sw:term_status "accepted"@en ;
    skos:definition "Data subjects that receive medical attention, treatment, care, advice, or other health related services"@en ;
    skos:prefLabel "Patient"@en .

dpv-owl:PaymentManagement a rdfs:Class,
        owl:Class,
        dpv-owl:Purpose ;
    dct:contributor "Georg P. Krog, Harshvardhan J. Pandit, Beatriz Esteves" ;
    dct:created "2020-11-04"^^xsd:date ;
    rdfs:isDefinedBy dpv-owl: ;
    rdfs:subClassOf dpv-owl:ServiceProvision ;
    sw:term_status "accepted"@en ;
    skos:definition "Purposes associated with processing and managing payment in relation to service, including invoicing and records"@en ;
    skos:prefLabel "Payment Management"@en .

dpv-owl:PenetrationTestingMethods a rdfs:Class,
        owl:Class,
        dpv-owl:TechnicalMeasure ;
    dct:contributor "Harshvardhan J. Pandit" ;
    dct:created "2022-08-17"^^xsd:date ;
    dct:source [ a schema:WebPage ;
            schema:name "ENISA Reference Incident Classification Taxonomy 2018" ;
            schema:url "https://www.enisa.europa.eu/publications/reference-incident-classification-taxonomy/" ] ;
    rdfs:isDefinedBy dpv-owl: ;
    rdfs:subClassOf dpv-owl:SecurityMethod ;
    sw:term_status "accepted"@en ;
    skos:definition "Use of penetration testing to identify weaknesses and vulnerabilities through simulations"@en ;
    skos:prefLabel "Penetration Testing Methods"@en .

dpv-owl:Permission a rdfs:Class,
        owl:Class,
        dpv-owl:Rule ;
    dct:contributor "Harshvardhan J. Pandit, Georg P. Krog, Beatriz Esteves, Paul Ryan" ;
    dct:created "2022-10-19"^^xsd:date ;
    vann:example dex-owl:E0028,
        dex-owl:E0066 ;
    rdfs:isDefinedBy dpv-owl: ;
    rdfs:subClassOf dpv-owl:Rule ;
    sw:term_status "accepted"@en ;
    skos:definition "A rule describing a permission to perform an activity"@en ;
    skos:prefLabel "Permission"@en .

dpv-owl:PermissionManagement a rdfs:Class,
        owl:Class,
        dpv-owl:OrganisationalMeasure ;
    dct:contributor "Beatriz Esteves, Harshvardhan J. Pandit, Georg P. Krog" ;
    dct:created "2024-04-14"^^xsd:date ;
    dct:source "DGA 12.n"@en ;
    rdfs:isDefinedBy dpv-owl: ;
    rdfs:subClassOf dpv-owl:RightsManagement ;
    sw:term_status "accepted"@en ;
    skos:definition "Methods to obtain, provide, modify, and withdraw permissions along with maintaining a record of permissions, retrieving records, and processing changes in permission states"@en ;
    skos:prefLabel "Permission Management"@en ;
    skos:scopeNote "Permission is a broader concept than '(Informed) Consent' as consent when used as a legal basis has specific requirements to be valid. For management of consent, see the concept dpv:ConsentManagement"@en .

dpv-owl:PersonalData a rdfs:Class,
        owl:Class ;
    dct:contributor "Harshvardhan J. Pandit" ;
    dct:created "2019-04-05"^^xsd:date ;
    dct:modified "2022-01-19"^^xsd:date ;
    dct:source [ a schema:WebPage ;
            schema:name "GDPR Art.4-1g" ;
            schema:url "https://eur-lex.europa.eu/eli/reg/2016/679/art_4/par_1/oj" ] ;
    vann:example dex-owl:E0044 ;
    rdfs:isDefinedBy dpv-owl: ;
    rdfs:subClassOf dpv-owl:Data ;
    sw:term_status "accepted"@en ;
    skos:definition "Data directly or indirectly associated or related to an individual."@en ;
    skos:prefLabel "Personal Data"@en ;
    skos:related spl:AnyData ;
    skos:scopeNote "This definition of personal data encompasses the concepts used in GDPR Art.4-1 for 'personal data' and ISO/IEC 2700 for 'personally identifiable information (PII)'."@en .

dpv-owl:PersonalDataHandling a rdfs:Class,
        owl:Class ;
    dct:contributor "Axel Polleres, Javier Fernández" ;
    dct:created "2019-04-05"^^xsd:date ;
    dct:modified "2023-12-10"^^xsd:date ;
    rdfs:isDefinedBy dpv-owl: ;
    rdfs:subClassOf dpv-owl:Process ;
    sw:term_status "sunset"@en ;
    skos:definition "An abstract concept describing 'personal data handling'"@en ;
    skos:prefLabel "Personal Data Handling"@en ;
    skos:scopeNote "This concept will be deprecated in future updates. It is recommended to use dpv:Process as the equivalent alternative which is better aligned with legal and operational terminology."@en .

dpv-owl:PersonalDataProcess a rdfs:Class,
        owl:Class ;
    dct:contributor "Harshvardhan J. Pandit" ;
    dct:created "2024-05-09"^^xsd:date ;
    rdfs:isDefinedBy dpv-owl: ;
    rdfs:subClassOf dpv-owl:Process ;
    sw:term_status "accepted"@en ;
    skos:definition "An action, activity, or method involving personal data"@en ;
    skos:prefLabel "Personal Data Process"@en .

dpv-owl:Personalisation a rdfs:Class,
        owl:Class,
        dpv-owl:Purpose ;
    dct:contributor "Harshvardhan J. Pandit" ;
    dct:created "2021-09-01"^^xsd:date ;
    rdfs:isDefinedBy dpv-owl: ;
    rdfs:subClassOf dpv-owl:Purpose ;
    sw:term_status "accepted"@en ;
    skos:definition "Purposes associated with creating and providing customisation based on attributes and/or needs of person(s) or context(s)."@en ;
    skos:prefLabel "Personalisation"@en ;
    skos:scopeNote "This term is a blanket purpose category for indicating personalisation of some other purpose, e.g. by creating a subclass of the other concept and Personalisation"@en .

dpv-owl:PersonalisedAdvertising a rdfs:Class,
        owl:Class,
        dpv-owl:Purpose ;
    dct:contributor "Georg P. Krog, Harshvardhan J. Pandit, Beatriz Esteves" ;
    dct:created "2020-11-04"^^xsd:date ;
    rdfs:isDefinedBy dpv-owl: ;
    rdfs:subClassOf dpv-owl:Advertising,
        dpv-owl:Personalisation ;
    sw:term_status "accepted"@en ;
    skos:definition "Purposes associated with creating and providing personalised advertising"@en ;
    skos:prefLabel "Personalised Advertising"@en .

dpv-owl:PersonalisedBenefits a rdfs:Class,
        owl:Class,
        dpv-owl:Purpose ;
    dct:contributor "Harshvardhan J. Pandit, Javier Fernández, Axel Polleres, Elmar Kiesling, Fajar Ekaputra, Simon Steyskal" ;
    dct:created "2019-04-05"^^xsd:date ;
    rdfs:isDefinedBy dpv-owl: ;
    rdfs:subClassOf dpv-owl:ServicePersonalisation ;
    sw:term_status "accepted"@en ;
    skos:definition "Purposes associated with creating and providing personalised benefits for a service"@en ;
    skos:prefLabel "Personalised Benefits"@en .

dpv-owl:PersonnelHiring a rdfs:Class,
        owl:Class,
        dpv-owl:Purpose ;
    dct:contributor "Harshvardhan J. Pandit" ;
    dct:created "2022-04-20"^^xsd:date ;
    rdfs:isDefinedBy dpv-owl: ;
    rdfs:subClassOf dpv-owl:PersonnelManagement ;
    sw:term_status "accepted"@en ;
    skos:definition "Purposes associated with management and execution of hiring processes of personnel"@en ;
    skos:prefLabel "Personnel Hiring"@en .

dpv-owl:PersonnelManagement a rdfs:Class,
        owl:Class,
        dpv-owl:Purpose ;
    dct:contributor "Paul Ryan, Harshvardhan J. Pandit" ;
    dct:created "2022-03-30"^^xsd:date ;
    dct:source [ a schema:WebPage ;
            schema:name "Belgian DPA ROPA Template" ;
            schema:url "https://www.privacycommission.be/nl/model-voor-een-register-van-de-verwerkingsactiviteiten" ] ;
    rdfs:isDefinedBy dpv-owl: ;
    rdfs:subClassOf dpv-owl:HumanResourceManagement ;
    sw:term_status "accepted"@en ;
    skos:definition "Purposes associated with management of personnel associated with the organisation e.g. evaluation and management of employees and intermediaries"@en ;
    skos:prefLabel "Personnel Management"@en .

dpv-owl:PersonnelPayment a rdfs:Class,
        owl:Class,
        dpv-owl:Purpose ;
    dct:contributor "Harshvardhan J. Pandit" ;
    dct:created "2022-04-20"^^xsd:date ;
    rdfs:isDefinedBy dpv-owl: ;
    rdfs:subClassOf dpv-owl:PersonnelManagement ;
    sw:term_status "accepted"@en ;
    skos:definition "Purposes associated with management and execution of payment of personnel"@en ;
    skos:prefLabel "Personnel Payment"@en .

dpv-owl:PhysicalAccessControlMethod a rdfs:Class,
        owl:Class,
        dpv-owl:PhysicalMeasure ;
    dct:contributor "Georg P. Krog" ;
    dct:created "2022-06-15"^^xsd:date ;
    dct:source "NIST SP 800-12"@en ;
    rdfs:isDefinedBy dpv-owl: ;
    rdfs:subClassOf dpv-owl:AccessControlMethod ;
    sw:term_status "accepted"@en ;
    skos:definition "Access control applied for physical access e.g. premises or equipment"@en ;
    skos:prefLabel "Physical Access Control Method"@en .

dpv-owl:PhysicalAuthentication a rdfs:Class,
        owl:Class,
        dpv-owl:PhysicalMeasure ;
    dct:contributor "Harshvardhan J. Pandit" ;
    dct:created "2024-04-14"^^xsd:date ;
    dct:source "NIST SP 800-15"@en ;
    rdfs:isDefinedBy dpv-owl: ;
    rdfs:subClassOf dpv-owl:PhysicalMeasure ;
    sw:term_status "accepted"@en ;
    skos:definition "Physical implementation of authentication e.g. by matching the person to their ID card"@en ;
    skos:prefLabel "Physical Authentication"@en .

dpv-owl:PhysicalAuthorisation a rdfs:Class,
        owl:Class,
        dpv-owl:PhysicalMeasure ;
    dct:contributor "Harshvardhan J. Pandit" ;
    dct:created "2024-04-14"^^xsd:date ;
    dct:source "NIST SP 800-16"@en ;
    rdfs:isDefinedBy dpv-owl: ;
    rdfs:subClassOf dpv-owl:PhysicalMeasure ;
    sw:term_status "accepted"@en ;
    skos:definition "Physical implementation of authorisation e.g. by stamping a visitor pass"@en ;
    skos:prefLabel "Physical Authorisation"@en .

dpv-owl:PhysicalDeviceSecurity a rdfs:Class,
        owl:Class,
        dpv-owl:PhysicalMeasure ;
    dct:contributor "Harshvardhan J. Pandit" ;
    dct:created "2024-04-14"^^xsd:date ;
    dct:source "NIST SP 800-19"@en ;
    rdfs:isDefinedBy dpv-owl: ;
    rdfs:subClassOf dpv-owl:PhysicalMeasure ;
    sw:term_status "accepted"@en ;
    skos:definition "Physical protection for devices and equipment"@en ;
    skos:prefLabel "Physical Device Security"@en .

dpv-owl:PhysicalInterceptionProtection a rdfs:Class,
        owl:Class,
        dpv-owl:PhysicalMeasure ;
    dct:contributor "Harshvardhan J. Pandit" ;
    dct:created "2024-04-14"^^xsd:date ;
    dct:source "NIST SP 800-20"@en ;
    rdfs:isDefinedBy dpv-owl: ;
    rdfs:subClassOf dpv-owl:PhysicalMeasure ;
    sw:term_status "accepted"@en ;
    skos:definition "Physical protection against interception e.g. by posting a guard"@en ;
    skos:prefLabel "Physical Interception Protection"@en .

dpv-owl:PhysicalInterruptionProtection a rdfs:Class,
        owl:Class,
        dpv-owl:PhysicalMeasure ;
    dct:contributor "Harshvardhan J. Pandit" ;
    dct:created "2024-04-14"^^xsd:date ;
    dct:source "NIST SP 800-18"@en ;
    rdfs:isDefinedBy dpv-owl: ;
    rdfs:subClassOf dpv-owl:PhysicalMeasure ;
    sw:term_status "accepted"@en ;
    skos:definition "Physical protection against interruptions e.g. electrical supply interruption"@en ;
    skos:prefLabel "Physical Interruption Protection"@en .

dpv-owl:PhysicalMeasure a rdfs:Class,
        owl:Class ;
    dct:created "2023-12-10"^^xsd:date ;
    dct:modified "2023-12-10"^^xsd:date ;
    rdfs:isDefinedBy dpv-owl: ;
    rdfs:subClassOf dpv-owl:TechnicalOrganisationalMeasure ;
    sw:term_status "accepted"@en ;
    skos:definition "Physical measures used to safeguard and ensure good practices in connection with data and technologies"@en ;
    skos:prefLabel "Physical Measure"@en .

dpv-owl:PhysicalNetworkSecurity a rdfs:Class,
        owl:Class,
        dpv-owl:PhysicalMeasure ;
    dct:contributor "Harshvardhan J. Pandit" ;
    dct:created "2024-04-14"^^xsd:date ;
    dct:source "NIST SP 800-17"@en ;
    rdfs:isDefinedBy dpv-owl: ;
    rdfs:subClassOf dpv-owl:PhysicalMeasure ;
    sw:term_status "accepted"@en ;
    skos:definition "Physical protection for networks and networking related infrastructure e.g. by isolating networking equipments"@en ;
    skos:prefLabel "Physical Network Security"@en .

dpv-owl:PhysicalSecureStorage a rdfs:Class,
        owl:Class,
        dpv-owl:PhysicalMeasure ;
    dct:contributor "Harshvardhan J. Pandit" ;
    dct:created "2024-04-14"^^xsd:date ;
    dct:source "NIST SP 800-171"@en ;
    rdfs:isDefinedBy dpv-owl: ;
    rdfs:subClassOf dpv-owl:PhysicalMeasure ;
    sw:term_status "accepted"@en ;
    skos:definition "Physical protection for storage of information or equipment e.g. secure storage for files"@en ;
    skos:prefLabel "Physical Secure Storage"@en .

dpv-owl:PhysicalSupplySecurity a rdfs:Class,
        owl:Class,
        dpv-owl:PhysicalMeasure ;
    dct:contributor "Harshvardhan J. Pandit" ;
    dct:created "2024-04-14"^^xsd:date ;
    dct:source "NIST SP 800-14"@en ;
    rdfs:isDefinedBy dpv-owl: ;
    rdfs:subClassOf dpv-owl:PhysicalMeasure ;
    sw:term_status "accepted"@en ;
    skos:definition "Physically securing the supply of resources"@en ;
    skos:prefLabel "Physical Supply Security"@en .

dpv-owl:PhysicalSurveillance a rdfs:Class,
        owl:Class,
        dpv-owl:PhysicalMeasure ;
    dct:contributor "Harshvardhan J. Pandit" ;
    dct:created "2024-04-14"^^xsd:date ;
    dct:source "NIST SP 800-171"@en ;
    rdfs:isDefinedBy dpv-owl: ;
    rdfs:subClassOf dpv-owl:PhysicalMeasure ;
    sw:term_status "accepted"@en ;
    skos:definition "Physically monitoring areas via surveillance"@en ;
    skos:prefLabel "Physical Surveillance"@en .

dpv-owl:Policy a rdfs:Class,
        owl:Class,
        dpv-owl:OrganisationalMeasure ;
    dct:contributor "Paul Ryan, David Hickey, Georg P. Krog, Harshvardhan J. Pandit" ;
    dct:created "2021-09-08"^^xsd:date ;
    rdfs:isDefinedBy dpv-owl: ;
    rdfs:subClassOf dpv-owl:GovernanceProcedures ;
    sw:term_status "accepted"@en ;
    skos:definition "A guidance document outlining any of: procedures, plans, principles, decisions, intent, or protocols."@en ;
    skos:prefLabel "Policy"@en .

dpv-owl:PostQuantumCryptography a rdfs:Class,
        owl:Class,
        dpv-owl:TechnicalMeasure ;
    dct:contributor "Harshvardhan J. Pandit" ;
    dct:created "2022-08-17"^^xsd:date ;
    dct:source [ a schema:WebPage ;
            schema:name "ENISA Reference Incident Classification Taxonomy 2018" ;
            schema:url "https://www.enisa.europa.eu/publications/reference-incident-classification-taxonomy/" ] ;
    rdfs:isDefinedBy dpv-owl: ;
    rdfs:subClassOf dpv-owl:CryptographicMethods ;
    sw:term_status "accepted"@en ;
    skos:definition "Use of algorithms that are intended to be secure against cryptanalytic attack by a quantum computer"@en ;
    skos:prefLabel "Post-Quantum Cryptography"@en .

dpv-owl:PrimaryImportance a rdfs:Class,
        owl:Class,
        dpv-owl:Importance ;
    dct:contributor "Harshvardhan J. Pandit, Paul Ryan, Georg P. Krog, Julian Flake, Beatriz Esteves" ;
    dct:created "2022-02-10"^^xsd:date ;
    rdfs:isDefinedBy dpv-owl: ;
    rdfs:subClassOf dpv-owl:Importance ;
    sw:term_status "accepted"@en ;
    skos:definition "Indication of 'primary' or 'main' or 'core' importance"@en ;
    skos:prefLabel "Primary Importance"@en .

dpv-owl:Principle a rdfs:Class,
        owl:Class,
        dpv-owl:OrganisationalMeasure ;
    dct:contributor "Harshvardhan J. Pandit" ;
    dct:created "2024-05-12"^^xsd:date ;
    rdfs:isDefinedBy dpv-owl: ;
    rdfs:subClassOf dpv-owl:GuidelinesPrinciple ;
    sw:term_status "accepted"@en ;
    skos:definition "A representation of values or norms that must be taken into consideration when conducting activities"@en ;
    skos:prefLabel "Principle"@en .

dpv-owl:PrivacyByDefault a rdfs:Class,
        owl:Class,
        dpv-owl:OrganisationalMeasure ;
    dct:contributor "Axel Polleres, Rob Brennan, Harshvardhan J. Pandit, Mark Lizar" ;
    dct:created "2019-04-05"^^xsd:date ;
    dct:modified "2024-04-14"^^xsd:date ;
    rdfs:isDefinedBy dpv-owl: ;
    rdfs:subClassOf dpv-owl:GuidelinesPrinciple ;
    sw:term_status "accepted"@en ;
    skos:definition "Practices regarding setting the default configurations of information and services to implement data protection and privacy (synonymous with Data Protection by Default)"@en ;
    skos:prefLabel "Privacy by Default"@en .

dpv-owl:PrivacyByDesign a rdfs:Class,
        owl:Class,
        dpv-owl:OrganisationalMeasure ;
    dct:contributor "Axel Polleres, Rob Brennan, Harshvardhan J. Pandit, Mark Lizar" ;
    dct:created "2019-04-05"^^xsd:date ;
    rdfs:isDefinedBy dpv-owl: ;
    rdfs:subClassOf dpv-owl:GuidelinesPrinciple ;
    sw:term_status "accepted"@en ;
    skos:definition "Practices regarding incorporating data protection and privacy in the design of information and services (synonymous with Data Protection by Design)"@en ;
    skos:prefLabel "Privacy by Design"@en .

dpv-owl:PrivacyNotice a rdfs:Class,
        owl:Class,
        dpv-owl:OrganisationalMeasure ;
    dct:contributor "Georg P. Krog, Paul Ryan, David Hickey, Harshvardhan J. Pandit" ;
    dct:created "2021-09-08"^^xsd:date ;
    vann:example dex-owl:E0017,
        dex-owl:E0022 ;
    rdfs:isDefinedBy dpv-owl: ;
    rdfs:subClassOf dpv-owl:Notice ;
    sw:term_status "accepted"@en ;
    skos:definition "Represents a notice or document outlining information regarding privacy"@en ;
    skos:prefLabel "Privacy Notice"@en .

dpv-owl:PrivacyPreservingProtocol a rdfs:Class,
        owl:Class,
        dpv-owl:TechnicalMeasure ;
    dct:contributor "Harshvardhan J. Pandit" ;
    dct:created "2022-08-17"^^xsd:date ;
    dct:source [ a schema:WebPage ;
            schema:name "ENISA Reference Incident Classification Taxonomy 2018" ;
            schema:url "https://www.enisa.europa.eu/publications/reference-incident-classification-taxonomy/" ] ;
    rdfs:isDefinedBy dpv-owl: ;
    rdfs:subClassOf dpv-owl:CryptographicMethods ;
    sw:term_status "accepted"@en ;
    skos:definition "Use of protocols designed with the intention of provided additional guarantees regarding privacy"@en ;
    skos:prefLabel "Privacy Preserving Protocol"@en .

dpv-owl:PrivateInformationRetrieval a rdfs:Class,
        owl:Class,
        dpv-owl:TechnicalMeasure ;
    dct:contributor "Harshvardhan J. Pandit" ;
    dct:created "2022-08-17"^^xsd:date ;
    dct:source [ a schema:WebPage ;
            schema:name "ENISA Data Protection Engineering" ;
            schema:url "https://www.enisa.europa.eu/publications/data-protection-engineering" ] ;
    rdfs:isDefinedBy dpv-owl: ;
    rdfs:subClassOf dpv-owl:CryptographicMethods ;
    sw:term_status "accepted"@en ;
    skos:definition "Use of cryptographic methods to retrieve a record from a system without revealing which record is retrieved"@en ;
    skos:prefLabel "Private Information Retrieval"@en .

dpv-owl:PrivateLocation a rdfs:Class,
        owl:Class,
        dpv-owl:Location ;
    dct:contributor "Harshvardhan J. Pandit" ;
    dct:created "2022-10-22"^^xsd:date ;
    rdfs:isDefinedBy dpv-owl: ;
    rdfs:subClassOf dpv-owl:LocalLocation ;
    sw:term_status "accepted"@en ;
    skos:definition "Location that is not or cannot be accessed by the public and is controlled as a private space"@en ;
    skos:prefLabel "Private Location"@en .

dpv-owl:Process a rdfs:Class,
        owl:Class ;
    dct:contributor "Harshvardhan J. Pandit" ;
    dct:created "2024-05-09"^^xsd:date ;
    vann:example dex-owl:E0005,
        dex-owl:E0006,
        dex-owl:E0031,
        dex-owl:E0041 ;
    rdfs:isDefinedBy dpv-owl: ;
    sw:term_status "accepted"@en ;
    skos:definition "An action, activity, or method"@en ;
    skos:prefLabel "Process"@en .

dpv-owl:Processing a rdfs:Class,
        owl:Class ;
    dct:contributor "Axel Polleres, Javier Fernández" ;
    dct:created "2019-04-05"^^xsd:date ;
    dct:modified "2020-11-04"^^xsd:date ;
    dct:source [ a schema:WebPage ;
            schema:name "SPECIAL Project" ;
            schema:url "https://specialprivacy.ercim.eu/" ] ;
    rdfs:isDefinedBy dpv-owl: ;
    sw:term_status "accepted"@en ;
    skos:definition "Operations or 'processing' performed on data"@en ;
    skos:prefLabel "Processing"@en ;
    skos:related spl:AnyProcessing .

dpv-owl:ProcessingCondition a rdfs:Class,
        owl:Class ;
    dct:created "2023-12-10"^^xsd:date ;
    vann:example dex-owl:E0047 ;
    rdfs:isDefinedBy dpv-owl: ;
    rdfs:subClassOf dpv-owl:ProcessingContext ;
    sw:term_status "accepted"@en ;
    skos:definition "Conditions required or followed regarding processing of data or use of technologies"@en ;
    skos:prefLabel "Processing Condition"@en .

dpv-owl:ProcessingContext a rdfs:Class,
        owl:Class ;
    dct:contributor "Harshvardhan J. Pandit" ;
    dct:created "2022-02-09"^^xsd:date ;
    rdfs:isDefinedBy dpv-owl: ;
    rdfs:subClassOf dpv-owl:Context ;
    sw:term_status "accepted"@en ;
    skos:definition "Context or conditions within which processing takes place"@en ;
    skos:prefLabel "Processing Context"@en .

dpv-owl:ProcessingDuration a rdfs:Class,
        owl:Class ;
    dct:created "2023-12-10"^^xsd:date ;
    dct:modified "2024-05-11"^^xsd:date ;
    vann:example dex-owl:E0047 ;
    rdfs:isDefinedBy dpv-owl: ;
    rdfs:subClassOf dpv-owl:Duration,
        dpv-owl:ProcessingCondition ;
    sw:term_status "accepted"@en ;
    skos:definition "Conditions regarding duration or temporal limitation for processing"@en ;
    skos:prefLabel "Processing Duration"@en .

dpv-owl:ProcessingLocation a rdfs:Class,
        owl:Class ;
    dct:created "2023-12-10"^^xsd:date ;
    dct:modified "2024-05-11"^^xsd:date ;
    vann:example dex-owl:E0047 ;
    rdfs:isDefinedBy dpv-owl: ;
    rdfs:subClassOf dpv-owl:Location,
        dpv-owl:ProcessingCondition ;
    sw:term_status "accepted"@en ;
    skos:definition "Conditions regarding location or geospatial scope where processing takes places"@en ;
    skos:prefLabel "Processing Location"@en .

dpv-owl:ProcessingScale a rdfs:Class,
        owl:Class ;
    dct:contributor "Harshvardhan J. Pandit, Piero Bonatti" ;
    dct:created "2022-09-07"^^xsd:date ;
    vann:example dex-owl:E0049 ;
    rdfs:isDefinedBy dpv-owl: ;
    rdfs:subClassOf dpv-owl:Scale ;
    sw:term_status "accepted"@en ;
    skos:definition "Scale of Processing"@en ;
    skos:prefLabel "Processing Scale"@en ;
    skos:scopeNote "The exact definition of what constitutes \"scale\" depends on use of jurisdictional, domain-specific, or other forms of externally defined criterias. Where possible, this should be reflected by extending the scales provided with the appropriate context."@en .

dpv-owl:ProfessionalTraining a rdfs:Class,
        owl:Class,
        dpv-owl:OrganisationalMeasure ;
    dct:contributor "Harshvardhan J. Pandit" ;
    dct:created "2022-08-17"^^xsd:date ;
    dct:source [ a schema:WebPage ;
            schema:name "ENISA Reference Incident Classification Taxonomy 2018" ;
            schema:url "https://www.enisa.europa.eu/publications/reference-incident-classification-taxonomy/" ] ;
    rdfs:isDefinedBy dpv-owl: ;
    rdfs:subClassOf dpv-owl:StaffTraining ;
    sw:term_status "accepted"@en ;
    skos:definition "Training methods that are intended to provide professional knowledge and expertise"@en ;
    skos:prefLabel "Professional Training"@en .

dpv-owl:Profiling a rdfs:Class,
        owl:Class,
        dpv-owl:Processing ;
    dct:created "2019-05-07"^^xsd:date ;
    dct:source [ a schema:WebPage ;
            schema:name "GDPR Art.4-2" ;
            schema:url "https://eur-lex.europa.eu/eli/reg/2016/679/art_4/par_2/oj" ] ;
    rdfs:isDefinedBy dpv-owl: ;
    rdfs:subClassOf dpv-owl:Use ;
    sw:term_status "accepted"@en ;
    skos:definition "to create a profile that describes or represents a person"@en ;
    skos:prefLabel "Profiling"@en .

dpv-owl:Prohibition a rdfs:Class,
        owl:Class,
        dpv-owl:Rule ;
    dct:contributor "Harshvardhan J. Pandit, Georg P. Krog, Beatriz Esteves, Paul Ryan" ;
    dct:created "2022-10-19"^^xsd:date ;
    vann:example dex-owl:E0029,
        dex-owl:E0066 ;
    rdfs:isDefinedBy dpv-owl: ;
    rdfs:subClassOf dpv-owl:Rule ;
    sw:term_status "accepted"@en ;
    skos:definition "A rule describing a prohibition to perform an activity"@en ;
    skos:prefLabel "Prohibition"@en .

dpv-owl:ProtectionOfIPR a rdfs:Class,
        owl:Class,
        dpv-owl:Purpose ;
    dct:contributor "Beatriz Esteves, Harshvardhan J. Pandit" ;
    dct:created "2024-02-14"^^xsd:date ;
    dct:source "DGA 3.1(c)"@en ;
    rdfs:isDefinedBy dpv-owl: ;
    rdfs:subClassOf dpv-owl:FulfilmentOfObligation ;
    sw:term_status "accepted"@en ;
    skos:definition "Purposes associated with the protection of intellectual property rights"@en ;
    skos:prefLabel "Protection of Intellectual Property Rights"@en .

dpv-owl:ProtectionOfNationalSecurity a rdfs:Class,
        owl:Class,
        dpv-owl:Purpose ;
    dct:contributor "Beatriz Esteves, Harshvardhan J. Pandit" ;
    dct:created "2024-02-14"^^xsd:date ;
    dct:source "DGA 1.5"@en ;
    rdfs:isDefinedBy dpv-owl: ;
    rdfs:subClassOf dpv-owl:PublicBenefit ;
    sw:term_status "accepted"@en ;
    skos:definition "Purposes associated with the protection of national security"@en ;
    skos:prefLabel "Protection of National Security"@en .

dpv-owl:ProtectionOfPublicSecurity a rdfs:Class,
        owl:Class,
        dpv-owl:Purpose ;
    dct:contributor "Beatriz Esteves, Harshvardhan J. Pandit" ;
    dct:created "2024-02-14"^^xsd:date ;
    dct:source "DGA 3.2(d)"@en ;
    rdfs:isDefinedBy dpv-owl: ;
    rdfs:subClassOf dpv-owl:PublicBenefit ;
    sw:term_status "accepted"@en ;
    skos:definition "Purposes associated with the protection of public security"@en ;
    skos:prefLabel "Protection of Public Security"@en .

dpv-owl:ProvideConsent a rdfs:Class,
        owl:Class ;
    dct:created "2024-05-11"^^xsd:date ;
    rdfs:isDefinedBy dpv-owl: ;
    rdfs:subClassOf dpv-owl:ConsentControl,
        dpv-owl:OptingInToProcess ;
    sw:term_status "accepted"@en ;
    skos:definition "Control for providing consent"@en ;
    skos:prefLabel "Provide Consent"@en ;
    skos:scopeNote "Indicates how the data subject can provide consent e.g. used with dpv:isExercisedAt"@en .

dpv-owl:ProvideEventRecommendations a rdfs:Class,
        owl:Class,
        dpv-owl:Purpose ;
    dct:contributor "Harshvardhan J. Pandit, Rudy Jacob" ;
    dct:created "2019-11-26"^^xsd:date ;
    dct:modified "2022-10-14"^^xsd:date ;
    dct:source [ a schema:WebPage ;
            schema:name "SPECIAL Project" ;
            schema:url "https://specialprivacy.ercim.eu/" ] ;
    rdfs:isDefinedBy dpv-owl: ;
    rdfs:subClassOf dpv-owl:ProvidePersonalisedRecommendations ;
    sw:term_status "accepted"@en ;
    skos:definition "Purposes associated with creating and providing personalised recommendations for events"@en ;
    skos:prefLabel "Provide Event Recommendations"@en .

dpv-owl:ProvideOfficialStatistics a rdfs:Class,
        owl:Class,
        dpv-owl:Purpose ;
    dct:contributor "Beatriz Esteves, Harshvardhan J. Pandit" ;
    dct:created "2024-02-14"^^xsd:date ;
    dct:source "DGA 2.16"@en ;
    rdfs:isDefinedBy dpv-owl: ;
    rdfs:subClassOf dpv-owl:PublicBenefit ;
    sw:term_status "accepted"@en ;
    skos:definition "Purposes associated with facilitating the development, production and dissemination of reliable official statistics"@en ;
    skos:prefLabel "Provide Official Statistics"@en .

dpv-owl:ProvidePersonalisedRecommendations a rdfs:Class,
        owl:Class,
        dpv-owl:Purpose ;
    dct:contributor "Harshvardhan J. Pandit, Rudy Jacob" ;
    dct:created "2019-11-26"^^xsd:date ;
    dct:modified "2022-10-14"^^xsd:date ;
    dct:source [ a schema:WebPage ;
            schema:name "SPECIAL Project" ;
            schema:url "https://specialprivacy.ercim.eu/" ] ;
    rdfs:isDefinedBy dpv-owl: ;
    rdfs:subClassOf dpv-owl:ServicePersonalisation ;
    sw:term_status "accepted"@en ;
    skos:definition "Purposes associated with creating and providing personalised recommendations"@en ;
    skos:prefLabel "Provide Personalised Recommendations"@en .

dpv-owl:ProvideProductRecommendations a rdfs:Class,
        owl:Class,
        dpv-owl:Purpose ;
    dct:contributor "Harshvardhan J. Pandit, Javier Fernández, Axel Polleres, Elmar Kiesling, Fajar Ekaputra, Simon Steyskal" ;
    dct:created "2019-04-05"^^xsd:date ;
    dct:modified "2022-10-14"^^xsd:date ;
    rdfs:isDefinedBy dpv-owl: ;
    rdfs:subClassOf dpv-owl:ProvidePersonalisedRecommendations ;
    sw:term_status "accepted"@en ;
    skos:definition "Purposes associated with creating and providing product recommendations e.g. suggest similar products"@en ;
    skos:prefLabel "Provide Product Recommendations"@en ;
    skos:related svpu:Marketing .

dpv-owl:ProvidedData a rdfs:Class,
        owl:Class ;
    dct:contributor "Harshvardhan J. Pandit, Paul Ryan" ;
    dct:created "2024-04-20"^^xsd:date ;
    rdfs:isDefinedBy dpv-owl: ;
    rdfs:subClassOf dpv-owl:CollectedData ;
    sw:term_status "accepted"@en ;
    skos:definition "Data that has been provided by an entity"@en ;
    skos:prefLabel "Provided Data"@en ;
    skos:scopeNote "Provided data involves one entity explicitly providing the data, which the other entity then collects"@en .

dpv-owl:ProvidedPersonalData a rdfs:Class,
        owl:Class ;
    dct:contributor "Harshvardhan J. Pandit, Paul Ryan" ;
    dct:created "2024-04-20"^^xsd:date ;
    vann:example dex-owl:E0046 ;
    rdfs:isDefinedBy dpv-owl: ;
    rdfs:subClassOf dpv-owl:CollectedPersonalData,
        dpv-owl:ProvidedData ;
    sw:term_status "accepted"@en ;
    skos:definition "Personal Data that has been provided by an entity such as the Data Subject"@en ;
    skos:prefLabel "Provided Personal Data"@en ;
    skos:scopeNote "Provided personal data involves one entity (e.g. data subject) explicitly providing the data, which the other entity (e.g. data controller) then collects"@en .

dpv-owl:Pseudonymisation a rdfs:Class,
        owl:Class,
        dpv-owl:TechnicalMeasure ;
    dct:contributor "Axel Polleres, Rob Brennan, Harshvardhan J. Pandit, Mark Lizar, Maya Borges, Damien Desfontaines" ;
    dct:created "2019-04-05"^^xsd:date ;
    dct:modified "2022-11-24"^^xsd:date ;
    dct:source [ a schema:WebPage ;
            schema:name "GDPR Art.4-5" ;
            schema:url "https://eur-lex.europa.eu/eli/reg/2016/679/art_4/par_5/oj" ] ;
    rdfs:isDefinedBy dpv-owl: ;
    rdfs:subClassOf dpv-owl:Deidentification ;
    sw:term_status "accepted"@en ;
    skos:definition "Pseudonymisation means the processing of personal data in such a manner that the personal data can no longer be attributed to a specific data subject without the use of additional information, provided that such additional information is kept separately and is subject to technical and organisational measures to ensure that the personal data are not attributed to an identified or identifiable natural person;"@en ;
    skos:prefLabel "Pseudonymisation"@en .

dpv-owl:Pseudonymise a rdfs:Class,
        owl:Class,
        dpv-owl:Processing ;
    dct:created "2019-05-07"^^xsd:date ;
    dct:modified "2022-10-14"^^xsd:date ;
    dct:source [ a schema:WebPage ;
            schema:name "GDPR Art.4-2" ;
            schema:url "https://eur-lex.europa.eu/eli/reg/2016/679/art_4/par_2/oj" ] ;
    rdfs:isDefinedBy dpv-owl: ;
    rdfs:subClassOf dpv-owl:Transform ;
    sw:term_status "accepted"@en ;
    skos:definition "to replace personal identifiable information by artificial identifiers"@en ;
    skos:prefLabel "Pseudonymise"@en .

dpv-owl:PseudonymisedData a rdfs:Class,
        owl:Class ;
    dct:contributor "Harshvardhan J. Pandit" ;
    dct:created "2022-01-19"^^xsd:date ;
    rdfs:isDefinedBy dpv-owl: ;
    rdfs:subClassOf dpv-owl:PersonalData ;
    sw:term_status "accepted"@en ;
    skos:definition "Pseudonymised Data is data that has gone a partial or incomplete anonymisation process by replacing the identifiable information with artificial identifiers or 'pseudonyms', and is still considered as personal data"@en ;
    skos:prefLabel "Pseudonymised Data"@en .

dpv-owl:PublicBenefit a rdfs:Class,
        owl:Class,
        dpv-owl:Purpose ;
    dct:contributor "Harshvardhan J. Pandit" ;
    dct:created "2024-02-14"^^xsd:date ;
    rdfs:isDefinedBy dpv-owl: ;
    rdfs:subClassOf dpv-owl:Purpose ;
    sw:term_status "accepted"@en ;
    skos:definition "Purposes undertaken and intended to provide benefit to public or society"@en ;
    skos:prefLabel "Public Benefit"@en .

dpv-owl:PublicDataSource a rdfs:Class,
        owl:Class,
        dpv-owl:DataSource ;
    dct:contributor "Georg P. Krog, Harshvardhan J. Pandit, Beatriz Esteves, Paul Ryan, Julian Flake" ;
    dct:created "2022-01-26"^^xsd:date ;
    rdfs:isDefinedBy dpv-owl: ;
    rdfs:subClassOf dpv-owl:DataSource ;
    sw:term_status "accepted"@en ;
    skos:definition "A source of data that is publicly accessible or available"@en ;
    skos:prefLabel "Public Data Source"@en ;
    skos:scopeNote "The term 'Public' is used here in a broad sense. Actual consideration of what is 'Public Data' can vary based on several contextual or jurisdictional factors such as  definition of open, methods of access, permissions and licenses."@en .

dpv-owl:PublicInterest a rdfs:Class,
        owl:Class,
        dpv-owl:LegalBasis ;
    dct:contributor "Harshvardhan J. Pandit" ;
    dct:created "2021-04-21"^^xsd:date ;
    rdfs:isDefinedBy dpv-owl: ;
    rdfs:subClassOf dpv-owl:LegalBasis ;
    sw:term_status "accepted"@en ;
    skos:definition "Activities are necessary or beneficial for interest of the public or society at large"@en ;
    skos:prefLabel "Public Interest"@en .

dpv-owl:PublicLocation a rdfs:Class,
        owl:Class,
        dpv-owl:Location ;
    dct:contributor "Georg P. Krog" ;
    dct:created "2022-10-22"^^xsd:date ;
    rdfs:isDefinedBy dpv-owl: ;
    rdfs:subClassOf dpv-owl:LocalLocation ;
    sw:term_status "accepted"@en ;
    skos:definition "Location that is or can be accessed by the public"@en ;
    skos:prefLabel "Public Location"@en .

dpv-owl:PublicPolicyMaking a rdfs:Class,
        owl:Class,
        dpv-owl:Purpose ;
    dct:contributor "Beatriz Esteves, Harshvardhan J. Pandit" ;
    dct:created "2024-02-14"^^xsd:date ;
    dct:source "DGA 2.16"@en ;
    rdfs:isDefinedBy dpv-owl: ;
    rdfs:subClassOf dpv-owl:PublicBenefit ;
    sw:term_status "accepted"@en ;
    skos:definition "Purposes associated with public policy making, such as the development of new laws"@en ;
    skos:prefLabel "Public Policy Making"@en .

dpv-owl:PublicRegisterOfEntities a rdfs:Class,
        owl:Class ;
    dct:contributor "Beatriz Esteves" ;
    dct:created "2024-06-11"^^xsd:date ;
    rdfs:isDefinedBy dpv-owl: ;
    sw:term_status "accepted"@en ;
    skos:definition "A publicly available list of entities e.g. to indicate which entities perform a certain activity within a certain location or jurisdiction"@en ;
    skos:prefLabel "Public Register of Entities"@en .

dpv-owl:PublicRelations a rdfs:Class,
        owl:Class,
        dpv-owl:Purpose ;
    dct:contributor "Paul Ryan, Georg P. Krog, David Hickey, Harshvardhan J. Pandit" ;
    dct:created "2021-09-01"^^xsd:date ;
    dct:source [ a schema:WebPage ;
            schema:name "Belgian DPA ROPA Template" ;
            schema:url "https://www.privacycommission.be/nl/model-voor-een-register-van-de-verwerkingsactiviteiten" ] ;
    rdfs:isDefinedBy dpv-owl: ;
    rdfs:subClassOf dpv-owl:Marketing ;
    sw:term_status "accepted"@en ;
    skos:definition "Purposes associated with managing and conducting public relations processes, including creating goodwill for the organisation"@en ;
    skos:prefLabel "Public Relations"@en .

dpv-owl:Purpose a rdfs:Class,
        owl:Class ;
    dct:contributor "Axel Polleres, Javier Fernández, Harshvardhan J. Pandit, Delaram Golpayegani" ;
    dct:created "2019-04-05"^^xsd:date ;
    dct:modified "2024-04-14"^^xsd:date ;
    dct:source [ a schema:WebPage ;
            schema:name "SPECIAL Project" ;
            schema:url "https://specialprivacy.ercim.eu/" ] ;
    vann:example dex-owl:E0003,
        dex-owl:E0004,
        dex-owl:E0007,
        dex-owl:E0008,
        dex-owl:E0040,
        dex-owl:E0041,
        dex-owl:E0042,
        dex-owl:E0043 ;
    rdfs:isDefinedBy dpv-owl: ;
    sw:term_status "accepted"@en ;
    skos:definition "Purpose or (broader) Goal associated with data or technology"@en ;
    skos:prefLabel "Purpose"@en ;
    skos:related spl:AnyPurpose ;
    skos:scopeNote "The purpose or goal here is intended to sufficiently describe the intention or objective of why the data or technology is being used, and should be broader than mere technical descriptions of achieving a capability. For example, \"Analyse Data\" is an abstract purpose with no indication of what the analyses is for as compared to a purpose such as \"Marketing\" or \"Service Provision\" which provide clarity and comprehension of the 'purpose' and can be enhanced with additional descriptions. Such modelling is in line with regulatory requirements regarding the specificity of purposes, for example in GDPR"@en .

dpv-owl:QuantumCryptography a rdfs:Class,
        owl:Class,
        dpv-owl:TechnicalMeasure ;
    dct:contributor "Harshvardhan J. Pandit" ;
    dct:created "2022-08-17"^^xsd:date ;
    dct:source [ a schema:WebPage ;
            schema:name "ENISA Reference Incident Classification Taxonomy 2018" ;
            schema:url "https://www.enisa.europa.eu/publications/reference-incident-classification-taxonomy/" ] ;
    rdfs:isDefinedBy dpv-owl: ;
    rdfs:subClassOf dpv-owl:CryptographicMethods ;
    sw:term_status "accepted"@en ;
    skos:definition "Cryptographic methods that utilise quantum mechanical properties to perform cryptographic tasks"@en ;
    skos:prefLabel "Quantum Cryptography"@en .

dpv-owl:Query a rdfs:Class,
        owl:Class,
        dpv-owl:Processing ;
    dct:contributor "Harshvardhan J. Pandit" ;
    dct:created "2022-06-15"^^xsd:date ;
    rdfs:isDefinedBy dpv-owl: ;
    rdfs:subClassOf dpv-owl:Consult ;
    sw:term_status "accepted"@en ;
    skos:definition "to query or make enquiries over data"@en ;
    skos:prefLabel "Query"@en .

dpv-owl:RNGPseudonymisation a rdfs:Class,
        owl:Class,
        dpv-owl:TechnicalMeasure ;
    dct:contributor "Harshvardhan J. Pandit" ;
    dct:created "2022-08-17"^^xsd:date ;
    dct:modified "2022-10-13"^^xsd:date ;
    dct:source [ a schema:WebPage ;
            schema:name "ENISA Data Pseudonymisation: Advanced Techniques and Use Cases" ;
            schema:url "https://www.enisa.europa.eu/publications/data-pseudonymisation-advanced-techniques-and-use-cases" ] ;
    rdfs:isDefinedBy dpv-owl: ;
    rdfs:subClassOf dpv-owl:Pseudonymisation ;
    sw:term_status "accepted"@en ;
    skos:definition "A pseudonymisation method where identifiers are substituted by a number chosen by a Random Number Generator (RNG)"@en ;
    skos:prefLabel "RNG Pseudonymisation"@en .

dpv-owl:ROPA a rdfs:Class,
        owl:Class,
        dpv-owl:OrganisationalMeasure ;
    dct:contributor "Georg P. Krog, Harshvardhan J. Pandit, Paul Ryan" ;
    dct:created "2021-09-08"^^xsd:date ;
    dct:modified "2024-04-14"^^xsd:date ;
    rdfs:isDefinedBy dpv-owl: ;
    rdfs:subClassOf dpv-owl:DataProcessingRecord ;
    sw:term_status "accepted"@en ;
    skos:definition "A Record of Processing Activities (ROPA) is a document detailing processing activities"@en ;
    skos:prefLabel "Records of Processing Activities"@en ;
    skos:scopeNote "ROPA under GDPR Art.30 has specific requirements regarding the information to be maintained. Additionally, Data Protection Authorities also provide additional information guidelines for information to be maintained in a ROPA. For more information see https://w3id.org/dpcat"@en .

dpv-owl:RandomLocation a rdfs:Class,
        owl:Class,
        dpv-owl:LocationFixture ;
    dct:contributor "Harshvardhan J. Pandit" ;
    dct:created "2022-06-15"^^xsd:date ;
    dct:modified "2020-10-05"^^xsd:date ;
    rdfs:isDefinedBy dpv-owl: ;
    rdfs:subClassOf dpv-owl:LocationFixture ;
    sw:term_status "accepted"@en ;
    skos:definition "Location that is random or unknown"@en ;
    skos:prefLabel "Random Location"@en .

dpv-owl:ReaffirmConsent a rdfs:Class,
        owl:Class ;
    dct:created "2024-05-11"^^xsd:date ;
    rdfs:isDefinedBy dpv-owl: ;
    rdfs:subClassOf dpv-owl:ConsentControl ;
    sw:term_status "accepted"@en ;
    skos:definition "Control for affirming consent"@en ;
    skos:prefLabel "Reaffirm Consent"@en ;
    skos:scopeNote "Indicates how the controller (with dpv:ObtainConsent) or data subject (with dpv:ProvideConsent) can reaffirm consent e.g. used with dpv:isExercisedAt"@en .

dpv-owl:RecertificationPolicy a rdfs:Class,
        owl:Class,
        dpv-owl:OrganisationalMeasure ;
    dct:created "2019-04-05"^^xsd:date ;
    dct:modified "2024-04-14"^^xsd:date ;
    rdfs:isDefinedBy dpv-owl: ;
    rdfs:subClassOf dpv-owl:Policy ;
    sw:term_status "accepted"@en ;
    skos:definition "Policy regarding repetition or renewal of existing certification(s)"@en ;
    skos:prefLabel "Recertification Policy"@en .

dpv-owl:Recipient a rdfs:Class,
        owl:Class ;
    dct:contributor "Axel Polleres, Javier Fernández" ;
    dct:created "2019-04-05"^^xsd:date ;
    dct:modified "2024-05-21"^^xsd:date ;
    dct:source [ a schema:WebPage ;
            schema:name "SPECIAL Project" ;
            schema:url "https://specialprivacy.ercim.eu/" ],
        [ a schema:WebPage ;
            schema:name "GDPR Art.4-9g" ;
            schema:url "https://eur-lex.europa.eu/eli/reg/2016/679/art_4/par_9/oj" ] ;
    rdfs:isDefinedBy dpv-owl: ;
    rdfs:subClassOf dpv-owl:LegalEntity ;
    sw:term_status "accepted"@en ;
    skos:definition "Entities that receive data or technologies"@en ;
    skos:prefLabel "Recipient"@en ;
    skos:related spl:AnyRecipient ;
    skos:scopeNote "Recipients that receive personal data can be a Third Party, Data Controller, or Data Processor."@en .

dpv-owl:RecipientInformed a rdfs:Class,
        owl:Class,
        dpv-owl:EntityInformedStatus ;
    dct:contributor "Harshvardhan J. Pandit, Delaram Golpayegani, Georg P. Krog, Paul Ryan" ;
    dct:created "2024-05-10"^^xsd:date ;
    rdfs:isDefinedBy dpv-owl: ;
    rdfs:subClassOf dpv-owl:EntityInformed ;
    sw:term_status "accepted"@en ;
    skos:definition "Status indicating Recipient has been informed about the specified context"@en ;
    skos:prefLabel "Recipient Informed"@en .

dpv-owl:RecipientUninformed a rdfs:Class,
        owl:Class,
        dpv-owl:EntityInformedStatus ;
    dct:contributor "Harshvardhan J. Pandit, Delaram Golpayegani, Georg P. Krog, Paul Ryan" ;
    dct:created "2024-05-10"^^xsd:date ;
    rdfs:isDefinedBy dpv-owl: ;
    rdfs:subClassOf dpv-owl:EntityUninformed ;
    sw:term_status "accepted"@en ;
    skos:definition "Status indicating Recipient is uninformed i.e. has not been informed about the specified context"@en ;
    skos:prefLabel "Recipient Uninformed"@en .

dpv-owl:Record a rdfs:Class,
        owl:Class,
        dpv-owl:Processing ;
    dct:created "2019-05-07"^^xsd:date ;
    dct:source [ a schema:WebPage ;
            schema:name "GDPR Art.4-2" ;
            schema:url "https://eur-lex.europa.eu/eli/reg/2016/679/art_4/par_2/oj" ] ;
    rdfs:isDefinedBy dpv-owl: ;
    rdfs:subClassOf dpv-owl:Obtain ;
    sw:term_status "accepted"@en ;
    skos:definition "to make a record (especially media)"@en ;
    skos:prefLabel "Record"@en .

dpv-owl:RecordManagement a rdfs:Class,
        owl:Class,
        dpv-owl:Purpose ;
    dct:contributor "Paul Ryan, Georg P. Krog, David Hickey, Harshvardhan J. Pandit" ;
    dct:created "2021-09-01"^^xsd:date ;
    rdfs:isDefinedBy dpv-owl: ;
    rdfs:subClassOf dpv-owl:Purpose ;
    sw:term_status "accepted"@en ;
    skos:definition "Purposes associated with manage creation, storage, and use of records relevant to operations, events, and processes e.g. to store logs or access requests"@en ;
    skos:prefLabel "Record Management"@en ;
    skos:scopeNote "This purpose relates specifically for record creation and management. This can be combined or used along with other purposes to express intentions such as records for legal compliance or vendor payments."@en .

dpv-owl:RecordsOfActivities a rdfs:Class,
        owl:Class,
        dpv-owl:OrganisationalMeasure ;
    dct:contributor "Georg P. Krog, Harshvardhan J. Pandit, Paul Ryan" ;
    dct:created "2021-09-08"^^xsd:date ;
    dct:modified "2024-05-05"^^xsd:date ;
    rdfs:isDefinedBy dpv-owl: ;
    rdfs:subClassOf dpv-owl:OrganisationalMeasure ;
    sw:term_status "accepted"@en ;
    skos:definition "Records of activities within some context such as maintenance tasks or governance functions"@en ;
    skos:prefLabel "Records of Activities"@en ;
    skos:scopeNote "Records can be any information associated with the activity e.g. logs, summaries."@en .

dpv-owl:Reformat a rdfs:Class,
        owl:Class,
        dpv-owl:Processing ;
    dct:contributor "Beatriz Esteves" ;
    dct:created "2024-04-14"^^xsd:date ;
    dct:source "DGA 12.d"@en ;
    rdfs:isDefinedBy dpv-owl: ;
    rdfs:subClassOf dpv-owl:Format ;
    sw:term_status "accepted"@en ;
    skos:definition "to rearrange or restructure data to change its form"@en ;
    skos:prefLabel "Reformat"@en .

dpv-owl:Region a rdfs:Class,
        owl:Class ;
    dct:contributor "Harshvardhan J. Pandit" ;
    dct:created "2022-01-19"^^xsd:date ;
    rdfs:isDefinedBy dpv-owl: ;
    rdfs:subClassOf dpv-owl:Country ;
    sw:term_status "accepted"@en ;
    skos:definition "A region is an area or site that is considered a location"@en ;
    skos:prefLabel "Region"@en .

dpv-owl:RegionalAuthority a rdfs:Class,
        owl:Class ;
    dct:contributor "Harshvardhan J. Pandit" ;
    dct:created "2022-02-02"^^xsd:date ;
    dct:source [ a schema:WebPage ;
            schema:name "ADMS controlled vocabulary" ;
            schema:url "http://purl.org/adms" ] ;
    rdfs:isDefinedBy dpv-owl: ;
    rdfs:subClassOf dpv-owl:Authority ;
    sw:term_status "accepted"@en ;
    skos:definition "An authority tasked with overseeing legal compliance for a region"@en ;
    skos:prefLabel "Regional Authority"@en .

dpv-owl:RegionalScale a rdfs:Class,
        owl:Class,
        dpv-owl:GeographicCoverage ;
    dct:contributor "Harshvardhan J. Pandit" ;
    dct:created "2022-06-15"^^xsd:date ;
    rdfs:isDefinedBy dpv-owl: ;
    rdfs:subClassOf dpv-owl:GeographicCoverage ;
    sw:term_status "accepted"@en ;
    skos:definition "Geographic coverage spanning a specific region or regions"@en ;
    skos:prefLabel "Regional Scale"@en .

dpv-owl:RegulatorySandbox a rdfs:Class,
        owl:Class,
        dpv-owl:OrganisationalMeasure ;
    dct:contributor "Harshvardhan J. Pandit" ;
    dct:created "2024-05-17"^^xsd:date ;
    dct:source [ a schema:WebPage ;
            schema:name "EU Council Regulatory sandboxes and experimentation clauses as tools for better regulation" ;
            schema:url "https://www.consilium.europa.eu/en/press/press-releases/2020/11/16/regulatory-sandboxes-and-experimentation-clauses-as-tools-for-better-regulation-council-adopts-conclusions/" ] ;
    rdfs:isDefinedBy dpv-owl: ;
    rdfs:subClassOf dpv-owl:Safeguard ;
    sw:term_status "accepted"@en ;
    skos:definition "Mechanism used by regulators and businesses for gauging the compatibility of regulations and innovative products, particularly in the context of digitalisation, in a controlled real-world environment with appropriate safeguards in place"@en ;
    skos:prefLabel "Regulatory Sandbox"@en .

dpv-owl:RemoteLocation a rdfs:Class,
        owl:Class,
        dpv-owl:Location ;
    dct:contributor "Harshvardhan J. Pandit" ;
    dct:created "2022-06-15"^^xsd:date ;
    dct:modified "2020-10-05"^^xsd:date ;
    rdfs:isDefinedBy dpv-owl: ;
    rdfs:subClassOf dpv-owl:LocationLocality ;
    sw:term_status "accepted"@en ;
    skos:definition "Location is remote i.e. not local"@en ;
    skos:prefLabel "Remote Location"@en .

dpv-owl:Remove a rdfs:Class,
        owl:Class,
        dpv-owl:Processing ;
    dct:created "2019-05-07"^^xsd:date ;
    dct:source [ a schema:WebPage ;
            schema:name "GDPR Art.4-2" ;
            schema:url "https://eur-lex.europa.eu/eli/reg/2016/679/art_4/par_2/oj" ] ;
    rdfs:isDefinedBy dpv-owl: ;
    rdfs:subClassOf dpv-owl:Processing ;
    sw:term_status "accepted"@en ;
    skos:definition "to destruct or erase data"@en ;
    skos:prefLabel "Remove"@en .

dpv-owl:RenewedConsentGiven a rdfs:Class,
        owl:Class,
        dpv-owl:ConsentStatus ;
    dct:contributor "Georg P. Krog, Harshvardhan J. Pandit, Paul Ryan, Julian Flake" ;
    dct:created "2022-06-22"^^xsd:date ;
    dct:source [ a schema:WebPage ;
            schema:name "GConsent" ;
            schema:url "https://w3id.org/GConsent" ] ;
    rdfs:isDefinedBy dpv-owl: ;
    rdfs:subClassOf dpv-owl:ConsentStatusValidForProcessing ;
    sw:term_status "accepted"@en ;
    skos:definition "The state where a previously given consent has been 'renewed' or 'refreshed' or 'reaffirmed' to form a new instance of given consent"@en ;
    skos:prefLabel "Renewed Consent Given"@en ;
    skos:scopeNote "An example of this state is when a previously given consent has expired, and the individual is presented a notice regarding continuing associated processing operations - to which they agree. This state can be useful to keep track of 'reconfirmed' or 'refreshed' consent within consent records, assist notices and contextual agents to create better consenting dialogues, and assist with specific legal obligations related to subsequent consenting"@en .

dpv-owl:RepairImpairments a rdfs:Class,
        owl:Class,
        dpv-owl:Purpose ;
    dct:contributor "Harshvardhan J. Pandit" ;
    dct:created "2022-08-24"^^xsd:date ;
    rdfs:isDefinedBy dpv-owl: ;
    rdfs:subClassOf dpv-owl:ServiceProvision ;
    sw:term_status "accepted"@en ;
    skos:definition "Purposes associated with identifying, rectifying, or otherwise undertaking activities intended to fix or repair impairments to existing functionalities"@en ;
    skos:prefLabel "Repair Impairments"@en ;
    skos:scopeNote "An example of identifying and rectifying impairments is the process of finding and fixing errors in products, commonly referred to as debugging"@en .

dpv-owl:Representative a rdfs:Class,
        owl:Class ;
    dct:contributor "Georg P. Krog, Paul Ryan, Harshvardhan J. Pandit, Beatriz Esteves" ;
    dct:created "2020-11-04"^^xsd:date ;
    dct:source [ a schema:WebPage ;
            schema:name "GDPR Art.27" ;
            schema:url "https://eur-lex.europa.eu/eli/reg/2016/679/art_27/oj" ] ;
    vann:example dex-owl:E0019,
        dex-owl:E0032 ;
    rdfs:isDefinedBy dpv-owl: ;
    rdfs:subClassOf dpv-owl:LegalEntity ;
    sw:term_status "accepted"@en ;
    skos:definition "A representative of a legal entity"@en ;
    skos:prefLabel "Representative"@en .

dpv-owl:RequestAccepted a rdfs:Class,
        owl:Class,
        dpv-owl:RequestStatus ;
    dct:contributor "Harshvardhan J. Pandit" ;
    dct:created "2022-11-30"^^xsd:date ;
    rdfs:isDefinedBy dpv-owl: ;
    rdfs:subClassOf dpv-owl:RequestStatus ;
    sw:term_status "accepted"@en ;
    skos:definition "State of a request being accepted towards fulfilment"@en ;
    skos:prefLabel "Request Accepted"@en .

dpv-owl:RequestAcknowledged a rdfs:Class,
        owl:Class,
        dpv-owl:RequestStatus ;
    dct:contributor "Harshvardhan J. Pandit" ;
    dct:created "2022-11-30"^^xsd:date ;
    rdfs:isDefinedBy dpv-owl: ;
    rdfs:subClassOf dpv-owl:RequestStatus ;
    sw:term_status "accepted"@en ;
    skos:definition "State of a request being acknowledged"@en ;
    skos:prefLabel "Request Acknowledged"@en .

dpv-owl:RequestActionDelayed a rdfs:Class,
        owl:Class,
        dpv-owl:RequestStatus ;
    dct:contributor "Harshvardhan J. Pandit" ;
    dct:created "2022-11-30"^^xsd:date ;
    vann:example dex-owl:E0058 ;
    rdfs:isDefinedBy dpv-owl: ;
    rdfs:subClassOf dpv-owl:RequestStatus ;
    sw:term_status "accepted"@en ;
    skos:definition "State of a request being delayed towards fulfilment"@en ;
    skos:prefLabel "Request Action Delayed"@en .

dpv-owl:RequestFulfilled a rdfs:Class,
        owl:Class,
        dpv-owl:RequestStatus ;
    dct:contributor "Harshvardhan J. Pandit" ;
    dct:created "2022-11-30"^^xsd:date ;
    rdfs:isDefinedBy dpv-owl: ;
    rdfs:subClassOf dpv-owl:RequestStatus ;
    sw:term_status "accepted"@en ;
    skos:definition "State of a request being fulfilled"@en ;
    skos:prefLabel "Request Fulfilled"@en .

dpv-owl:RequestInitiated a rdfs:Class,
        owl:Class,
        dpv-owl:RequestStatus ;
    dct:contributor "Harshvardhan J. Pandit" ;
    dct:created "2022-11-30"^^xsd:date ;
    rdfs:isDefinedBy dpv-owl: ;
    rdfs:subClassOf dpv-owl:RequestStatus ;
    sw:term_status "accepted"@en ;
    skos:definition "State of a request being initiated"@en ;
    skos:prefLabel "Request Initiated"@en .

dpv-owl:RequestRejected a rdfs:Class,
        owl:Class,
        dpv-owl:RequestStatus ;
    dct:contributor "Harshvardhan J. Pandit" ;
    dct:created "2022-11-30"^^xsd:date ;
    rdfs:isDefinedBy dpv-owl: ;
    rdfs:subClassOf dpv-owl:RequestStatus ;
    sw:term_status "accepted"@en ;
    skos:definition "State of a request being rejected towards non-fulfilment"@en ;
    skos:prefLabel "Request Rejected"@en .

dpv-owl:RequestRequiredActionPerformed a rdfs:Class,
        owl:Class,
        dpv-owl:RequestStatus ;
    dct:contributor "Harshvardhan J. Pandit" ;
    dct:created "2022-11-30"^^xsd:date ;
    rdfs:isDefinedBy dpv-owl: ;
    rdfs:subClassOf dpv-owl:RequestStatus ;
    sw:term_status "accepted"@en ;
    skos:definition "State of a request's required action having been performed by the other party"@en ;
    skos:prefLabel "Request Required Action Performed"@en .

dpv-owl:RequestRequiresAction a rdfs:Class,
        owl:Class,
        dpv-owl:RequestStatus ;
    dct:contributor "Harshvardhan J. Pandit" ;
    dct:created "2022-11-30"^^xsd:date ;
    rdfs:isDefinedBy dpv-owl: ;
    rdfs:subClassOf dpv-owl:RequestStatus ;
    sw:term_status "accepted"@en ;
    skos:definition "State of a request requiring an action to be performed from another party"@en ;
    skos:prefLabel "Request Requires Action"@en .

dpv-owl:RequestStatus a rdfs:Class,
        owl:Class ;
    dct:contributor "Harshvardhan J. Pandit" ;
    dct:created "2022-11-30"^^xsd:date ;
    rdfs:isDefinedBy dpv-owl: ;
    rdfs:subClassOf dpv-owl:Status ;
    sw:term_status "accepted"@en ;
    skos:definition "Status associated with requests"@en ;
    skos:prefLabel "Request Status"@en .

dpv-owl:RequestStatusQuery a rdfs:Class,
        owl:Class,
        dpv-owl:RequestStatus ;
    dct:contributor "Harshvardhan J. Pandit" ;
    dct:created "2022-11-30"^^xsd:date ;
    rdfs:isDefinedBy dpv-owl: ;
    rdfs:subClassOf dpv-owl:RequestStatus ;
    sw:term_status "accepted"@en ;
    skos:definition "State of a request's status being queried"@en ;
    skos:prefLabel "Request Status Query"@en .

dpv-owl:RequestUnfulfilled a rdfs:Class,
        owl:Class,
        dpv-owl:RequestStatus ;
    dct:contributor "Harshvardhan J. Pandit" ;
    dct:created "2022-11-30"^^xsd:date ;
    rdfs:isDefinedBy dpv-owl: ;
    rdfs:subClassOf dpv-owl:RequestStatus ;
    sw:term_status "accepted"@en ;
    skos:definition "State of a request being unfulfilled"@en ;
    skos:prefLabel "Request Unfulfilled"@en .

dpv-owl:RequestedServiceProvision a rdfs:Class,
        owl:Class,
        dpv-owl:Purpose ;
    dct:contributor "Georg P. Krog, Harshvardhan J. Pandit, Beatriz Esteves" ;
    dct:created "2021-09-08"^^xsd:date ;
    rdfs:isDefinedBy dpv-owl: ;
    rdfs:subClassOf dpv-owl:ServiceProvision ;
    sw:term_status "accepted"@en ;
    skos:definition "Purposes associated with delivering services as requested by user or consumer"@en ;
    skos:prefLabel "Requested Service Provision"@en ;
    skos:scopeNote "The use of 'request' here includes where an user explicitly asks for the service and also when an established contract requires the provision of the service"@en .

dpv-owl:Required a rdfs:Class,
        owl:Class,
        dpv-owl:Necessity ;
    dct:contributor "Harshvardhan J. Pandit, Paul Ryan, Georg P. Krog, Julian Flake, Beatriz Esteves" ;
    dct:created "2022-02-13"^^xsd:date ;
    rdfs:isDefinedBy dpv-owl: ;
    rdfs:subClassOf dpv-owl:Necessity ;
    sw:term_status "accepted"@en ;
    skos:definition "Indication of 'required' or 'necessary'"@en ;
    skos:prefLabel "Required"@en .

dpv-owl:ResearchAndDevelopment a rdfs:Class,
        owl:Class,
        dpv-owl:Purpose ;
    dct:contributor "Harshvardhan J. Pandit, Javier Fernández, Axel Polleres, Elmar Kiesling, Fajar Ekaputra, Simon Steyskal" ;
    dct:created "2019-04-05"^^xsd:date ;
    rdfs:isDefinedBy dpv-owl: ;
    rdfs:subClassOf dpv-owl:Purpose ;
    sw:term_status "accepted"@en ;
    skos:definition "Purposes associated with conducting research and development for new methods, products, or services"@en ;
    skos:prefLabel "Research and Development"@en .

dpv-owl:ResidualRisk a rdfs:Class,
        owl:Class ;
    dct:contributor "Harshvardhan J. Pandit" ;
    dct:created "2024-06-16"^^xsd:date ;
    vann:example dex-owl:E0068 ;
    rdfs:isDefinedBy dpv-owl: ;
    rdfs:subClassOf dpv-owl:Risk ;
    sw:term_status "accepted"@en ;
    skos:definition "Risk remaining after treatment or mitigation"@en ;
    skos:prefLabel "Residual Risk"@en .

dpv-owl:Restrict a rdfs:Class,
        owl:Class,
        dpv-owl:Processing ;
    dct:created "2019-05-07"^^xsd:date ;
    dct:source [ a schema:WebPage ;
            schema:name "GDPR Art.4-2" ;
            schema:url "https://eur-lex.europa.eu/eli/reg/2016/679/art_4/par_2/oj" ] ;
    rdfs:isDefinedBy dpv-owl: ;
    rdfs:subClassOf dpv-owl:Transform ;
    sw:term_status "accepted"@en ;
    skos:definition "to apply a restriction on the processing of specific records"@en ;
    skos:prefLabel "Restrict"@en .

dpv-owl:Retrieve a rdfs:Class,
        owl:Class,
        dpv-owl:Processing ;
    dct:created "2019-05-07"^^xsd:date ;
    dct:source [ a schema:WebPage ;
            schema:name "GDPR Art.4-2" ;
            schema:url "https://eur-lex.europa.eu/eli/reg/2016/679/art_4/par_2/oj" ] ;
    rdfs:isDefinedBy dpv-owl: ;
    rdfs:subClassOf dpv-owl:Use ;
    sw:term_status "accepted"@en ;
    skos:definition "to retrieve data, often in an automated manner"@en ;
    skos:prefLabel "Retrieve"@en .

dpv-owl:ReversingProcessEffects a rdfs:Class,
        owl:Class,
        dpv-owl:EntityPermissiveInvolvement ;
    dct:contributor "Harshvardhan J. Pandit, Delaram Golpayegani, Steve Hickman" ;
    dct:created "2024-05-11"^^xsd:date ;
    rdfs:isDefinedBy dpv-owl: ;
    rdfs:subClassOf dpv-owl:EntityPermissiveInvolvement ;
    sw:term_status "accepted"@en ;
    skos:definition "Involvement where entity can reverse effects of specified context"@en ;
    skos:prefLabel "Reversing Process Effects"@en ;
    skos:scopeNote "Effects refer to consequences and impacts arising from the process or from the outputs of a process"@en .

dpv-owl:ReversingProcessInput a rdfs:Class,
        owl:Class,
        dpv-owl:EntityPermissiveInvolvement ;
    dct:contributor "Harshvardhan J. Pandit, Delaram Golpayegani, Steve Hickman" ;
    dct:created "2024-05-11"^^xsd:date ;
    rdfs:isDefinedBy dpv-owl: ;
    rdfs:subClassOf dpv-owl:EntityPermissiveInvolvement ;
    sw:term_status "accepted"@en ;
    skos:definition "Involvement where entity can reverse input of specified context"@en ;
    skos:prefLabel "Reversing Process Input"@en ;
    skos:scopeNote "Reversion can be considered a form of correction in some instances. We welcome inputs to further explore and define this relation between correction and reversion concepts."@en .

dpv-owl:ReversingProcessOutput a rdfs:Class,
        owl:Class,
        dpv-owl:EntityPermissiveInvolvement ;
    dct:contributor "Harshvardhan J. Pandit, Delaram Golpayegani, Steve Hickman" ;
    dct:created "2024-05-11"^^xsd:date ;
    rdfs:isDefinedBy dpv-owl: ;
    rdfs:subClassOf dpv-owl:EntityPermissiveInvolvement ;
    sw:term_status "accepted"@en ;
    skos:definition "Involvement where entity can reverse output of specified context"@en ;
    skos:prefLabel "Reversing Process Output"@en ;
    skos:scopeNote "Reversing of outputs indicate discarding the output and going back to the previous output. This is different from correction of output which allows modification of the output - implying continuation of the process."@en .

dpv-owl:ReviewImpactAssessment a rdfs:Class,
        owl:Class,
        dpv-owl:OrganisationalMeasure ;
    dct:contributor "Harshvardhan J. Pandit, Georg P. Krog" ;
    dct:created "2022-10-22"^^xsd:date ;
    rdfs:isDefinedBy dpv-owl: ;
    rdfs:subClassOf dpv-owl:ImpactAssessment,
        dpv-owl:ReviewProcedure ;
    sw:term_status "accepted"@en ;
    skos:definition "Procedures to review impact assessments in terms of continued validity, adequacy for intended purposes, and conformance of processes with findings"@en ;
    skos:prefLabel "Review Impact Assessment"@en .

dpv-owl:ReviewProcedure a rdfs:Class,
        owl:Class,
        dpv-owl:OrganisationalMeasure ;
    dct:contributor "Harshvardhan J. Pandit, Georg P. Krog" ;
    dct:created "2022-10-22"^^xsd:date ;
    rdfs:isDefinedBy dpv-owl: ;
    rdfs:subClassOf dpv-owl:GovernanceProcedures ;
    sw:term_status "accepted"@en ;
    skos:definition "A procedure or process that reviews the correctness and validity of other procedures and policies e.g. to ensure continued validity, adequacy for intended purposes, and conformance of processes with findings"@en ;
    skos:prefLabel "Review Procedure"@en .

dpv-owl:Right a rdfs:Class,
        owl:Class ;
    dct:contributor "Harshvardhan J. Pandit, Beatriz Esteves, Georg P. Krog" ;
    dct:created "2020-11-18"^^xsd:date ;
    vann:example dex-owl:E0067 ;
    rdfs:isDefinedBy dpv-owl: ;
    sw:term_status "accepted"@en ;
    skos:definition "The right(s) applicable, provided, or expected"@en ;
    skos:prefLabel "Right"@en ;
    skos:scopeNote "A 'right' is a legal, social, or ethical principle of freedom or entitlement which dictate the norms regarding what is allowed or owed. Rights as a concept encompass a broad area of norms and entities, and are not specific to Individuals or Data Protection / Privacy. For individual specific rights, see dpv:DataSubjectRight"@en .

dpv-owl:RightExerciseActivity a rdfs:Class,
        owl:Class,
        dpv-owl:OrganisationalMeasure ;
    dct:contributor "Harshvardhan J. Pandit, Beatriz Esteves, Georg P. Krog, Paul Ryan" ;
    dct:created "2022-11-02"^^xsd:date ;
    vann:example dex-owl:E0059 ;
    rdfs:isDefinedBy dpv-owl: ;
    rdfs:subClassOf dpv-owl:OrganisationalMeasure ;
    sw:term_status "accepted"@en ;
    skos:definition "An activity representing an exercising of an active right"@en ;
    skos:prefLabel "Right Exercise Activity"@en ;
    skos:scopeNote "There may be multiple activities associated with exercising and fulfilling rights. See the RightExerciseRecord concept for record-keeping of such activities in a cohesive manner."@en .

dpv-owl:RightExerciseNotice a rdfs:Class,
        owl:Class,
        dpv-owl:OrganisationalMeasure ;
    dct:contributor "Harshvardhan J. Pandit, Beatriz Esteves, Georg P. Krog, Paul Ryan" ;
    dct:created "2022-10-22"^^xsd:date ;
    rdfs:isDefinedBy dpv-owl: ;
    rdfs:subClassOf dpv-owl:RightNotice ;
    sw:term_status "accepted"@en ;
    skos:definition "Information associated with exercising of an active right such as where and how to exercise the right, information required for it, or updates on an exercised rights request"@en ;
    skos:prefLabel "Right Exercise Notice"@en ;
    skos:scopeNote "This concept is intended for providing information regarding a right exercise. For specific instances of such exercises, see RightExerciseActivity and RightExerciseRecord."@en .

dpv-owl:RightExerciseRecord a rdfs:Class,
        owl:Class,
        dpv-owl:OrganisationalMeasure ;
    dct:contributor "Harshvardhan J. Pandit, Beatriz Esteves, Georg P. Krog, Paul Ryan" ;
    dct:created "2022-11-02"^^xsd:date ;
    vann:example dex-owl:E0057 ;
    rdfs:isDefinedBy dpv-owl: ;
    rdfs:subClassOf dpv-owl:Record ;
    sw:term_status "accepted"@en ;
    skos:definition "Record of a Right being exercised"@en ;
    skos:prefLabel "Right Exercise Record"@en ;
    skos:scopeNote "This concept represents a record of one or more right exercise activities, such as those associated with a single data subject or service or entity"@en .

dpv-owl:RightFulfilmentNotice a rdfs:Class,
        owl:Class,
        dpv-owl:OrganisationalMeasure ;
    dct:contributor "Harshvardhan J. Pandit, Beatriz Esteves" ;
    dct:created "2022-11-02"^^xsd:date ;
    rdfs:isDefinedBy dpv-owl: ;
    rdfs:subClassOf dpv-owl:RightExerciseNotice ;
    sw:term_status "accepted"@en ;
    skos:definition "Notice provided regarding fulfilment of a right"@en ;
    skos:prefLabel "Right Fulfilment Notice"@en ;
    skos:scopeNote "This notice is associated with situations where information is provided with the intention of progressing the fulfilment of a right. For example, a notice asking for more information regarding the scope of the right, or providing information on where to access the data provided under a right."@en .

dpv-owl:RightNonFulfilmentNotice a rdfs:Class,
        owl:Class,
        dpv-owl:OrganisationalMeasure ;
    dct:contributor "Harshvardhan J. Pandit, Beatriz Esteves" ;
    dct:created "2022-11-02"^^xsd:date ;
    vann:example dex-owl:E0058,
        dex-owl:E0061 ;
    rdfs:isDefinedBy dpv-owl: ;
    rdfs:subClassOf dpv-owl:RightExerciseNotice ;
    sw:term_status "accepted"@en ;
    skos:definition "Notice provided regarding non-fulfilment of a right"@en ;
    skos:prefLabel "Right Non-Fulfilment Notice"@en ;
    skos:scopeNote "This notice is associated with situations where information is provided with the intention of communicating non-fulfilment of a right. For example, to provide justifications on why a right could not be fulfilled or providing information about another entity  who should be approached for exercising this right."@en .

dpv-owl:RightNotice a rdfs:Class,
        owl:Class,
        dpv-owl:OrganisationalMeasure ;
    dct:contributor "Harshvardhan J. Pandit" ;
    dct:created "2024-06-16"^^xsd:date ;
    rdfs:isDefinedBy dpv-owl: ;
    rdfs:subClassOf dpv-owl:Notice ;
    sw:term_status "accepted"@en ;
    skos:definition "Information associated with rights, such as which rights exist, when and where they are applicable, and other relevant information"@en ;
    skos:prefLabel "Right Notice"@en ;
    skos:scopeNote "This concept also covers information about rights exercise, with dpv:RightExerciseNotice specifically representing information provided in connection with exercising of rights. Both notices may be needed, e.g. RightNotice for providing information about existence and exercise of rights, and RightExerciseNotice for providing additional information specifically about exercise of rights - such as to request more information or provide updates on an exercised rights request"@en .

dpv-owl:RightsFulfillment a rdfs:Class,
        owl:Class,
        dpv-owl:Purpose ;
    dct:contributor "Beatriz Esteves, Georg P. Krog, Harshvardhan J. Pandit" ;
    dct:created "2024-02-14"^^xsd:date ;
    rdfs:isDefinedBy dpv-owl: ;
    rdfs:subClassOf dpv-owl:LegalObligation ;
    sw:term_status "accepted"@en ;
    skos:definition "Purposes associated with the fulfillment of rights specified in law"@en ;
    skos:prefLabel "Rights Fulfillment"@en ;
    skos:scopeNote "Where Rights Fulfillment includes activities that are not legal obligations, for example conducting Identity Verification, the documentation should indicate this by expressing them as separate purposes within the same activity"@en .

dpv-owl:RightsImpactAssessment a rdfs:Class,
        owl:Class,
        dpv-owl:OrganisationalMeasure ;
    dct:contributor "Harshvardhan J. Pandit" ;
    dct:created "2024-04-14"^^xsd:date ;
    rdfs:isDefinedBy dpv-owl: ;
    rdfs:subClassOf dpv-owl:ImpactAssessment ;
    sw:term_status "accepted"@en ;
    skos:definition "Impact assessment which involves determining the impact on rights and freedoms"@en ;
    skos:prefLabel "Rights Impact Assessment"@en ;
    skos:scopeNote "The rights and freedoms may be those defined in law or other norms, and may be bound to a jurisdiction"@en .

dpv-owl:RightsManagement a rdfs:Class,
        owl:Class,
        dpv-owl:OrganisationalMeasure ;
    dct:contributor "Beatriz Esteves, Harshvardhan J. Pandit, Georg P. Krog" ;
    dct:created "2024-04-14"^^xsd:date ;
    rdfs:isDefinedBy dpv-owl: ;
    rdfs:subClassOf dpv-owl:OrganisationalMeasure ;
    sw:term_status "accepted"@en ;
    skos:definition "Methods associated with rights management where 'rights' refer to controlling who can do what with a resource"@en ;
    skos:prefLabel "Rights Management"@en .

dpv-owl:Risk a rdfs:Class,
        owl:Class ;
    dct:contributor "Harshvardhan J. Pandit" ;
    dct:created "2020-11-18"^^xsd:date ;
    vann:example dex-owl:E0027,
        dex-owl:E0068,
        dex-owl:E0071 ;
    rdfs:isDefinedBy dpv-owl: ;
    sw:term_status "accepted"@en ;
    skos:definition "A risk or possibility or uncertainty of negative effects, impacts, or consequences"@en ;
    skos:prefLabel "Risk"@en ;
    skos:scopeNote "Risks can be associated with one or more different concepts such as purpose, processing, personal data, technical or organisational measure"@en .

dpv-owl:RiskAssessment a rdfs:Class,
        owl:Class,
        dpv-owl:OrganisationalMeasure ;
    dct:contributor "Harshvardhan J. Pandit" ;
    dct:created "2024-04-14"^^xsd:date ;
    rdfs:isDefinedBy dpv-owl: ;
    rdfs:subClassOf dpv-owl:Assessment ;
    sw:term_status "accepted"@en ;
    skos:definition "Assessment involving identification, analysis, and evaluation of risk"@en ;
    skos:prefLabel "Risk Assessment"@en .

dpv-owl:RiskLevel a rdfs:Class,
        owl:Class ;
    dct:contributor "Harshvardhan J. Pandit" ;
    dct:created "2022-07-20"^^xsd:date ;
    vann:example dex-owl:E0068,
        dex-owl:E0071 ;
    rdfs:isDefinedBy dpv-owl: ;
    sw:term_status "accepted"@en ;
    skos:definition "The magnitude of a risk expressed as an indication to aid in its management"@en ;
    skos:prefLabel "Risk Level"@en ;
    skos:scopeNote "Risk Levels can be defined as a combination of different characteristics. For example, ISO 31073:2022 defines it as a combination of consequences and their likelihood. Another example would be the Risk Matrix where Risk Level is defined as a combination of Likelihood and Severity associated with the Risk."@en .

dpv-owl:RiskMitigationMeasure a rdfs:Class,
        owl:Class ;
    dct:contributor "Georg P. Krog, Harshvardhan J. Pandit, Paul Ryan" ;
    dct:created "2020-11-04"^^xsd:date ;
    vann:example dex-owl:E0068 ;
    rdfs:isDefinedBy dpv-owl: ;
    rdfs:subClassOf dpv-owl:TechnicalOrganisationalMeasure ;
    sw:term_status "accepted"@en ;
    skos:definition "Measures intended to mitigate, minimise, or prevent risk."@en ;
    skos:prefLabel "Risk Mitigation Measure"@en .

dpv-owl:Rule a rdfs:Class,
        owl:Class ;
    dct:contributor "Harshvardhan J. Pandit, Georg P. Krog, Beatriz Esteves, Paul Ryan" ;
    dct:created "2022-10-19"^^xsd:date ;
    vann:example dex-owl:E0030 ;
    rdfs:isDefinedBy dpv-owl: ;
    sw:term_status "accepted"@en ;
    skos:definition "A rule describing a process or control that directs or determines if and how an activity should be conducted"@en ;
    skos:prefLabel "Rule"@en .

dpv-owl:Safeguard a rdfs:Class,
        owl:Class,
        dpv-owl:OrganisationalMeasure ;
    dct:contributor "David Hickey, Paul Ryan, Georg P. Krog, Harshvardhan J. Pandit" ;
    dct:created "2021-09-22"^^xsd:date ;
    rdfs:isDefinedBy dpv-owl: ;
    rdfs:subClassOf dpv-owl:OrganisationalMeasure ;
    sw:term_status "accepted"@en ;
    skos:definition "A safeguard is a precautionary measure for the protection against or mitigation of negative effects"@en ;
    skos:prefLabel "Safeguard"@en ;
    skos:scopeNote "This concept is relevant given the requirement to assert safeguards in cross-border data transfers"@en .

dpv-owl:SafeguardForDataTransfer a rdfs:Class,
        owl:Class,
        dpv-owl:OrganisationalMeasure ;
    dct:contributor "David Hickey, Paul Ryan, Georg P. Krog, Harshvardhan J. Pandit" ;
    dct:created "2021-09-22"^^xsd:date ;
    rdfs:isDefinedBy dpv-owl: ;
    rdfs:subClassOf dpv-owl:Safeguard ;
    sw:term_status "accepted"@en ;
    skos:definition "Represents a safeguard used for data transfer. Can include technical or organisational measures."@en ;
    skos:prefLabel "Safeguard for Data Transfer"@en .

dpv-owl:Scale a rdfs:Class,
        owl:Class ;
    dct:contributor "Harshvardhan J. Pandit, Georg P. Krog, Rana Saniei" ;
    dct:created "2022-06-15"^^xsd:date ;
    rdfs:isDefinedBy dpv-owl: ;
    rdfs:subClassOf dpv-owl:ProcessingContext ;
    sw:term_status "accepted"@en ;
    skos:definition "A measurement along some dimension"@en ;
    skos:prefLabel "Scale"@en ;
    skos:scopeNote "Scales are subjective concepts that need to be defined and interpreted within the context of their application. For example, what would be small within one context could be large within another."@en .

dpv-owl:ScientificResearch a rdfs:Class,
        owl:Class,
        dpv-owl:Purpose ;
    dct:contributor "Beatriz Esteves, Harshvardhan J. Pandit" ;
    dct:created "2024-02-14"^^xsd:date ;
    dct:source "DGA 2.16"@en ;
    rdfs:isDefinedBy dpv-owl: ;
    rdfs:subClassOf dpv-owl:ResearchAndDevelopment ;
    sw:term_status "accepted"@en ;
    skos:definition "Purposes associated with scientific research"@en ;
    skos:prefLabel "Scientific Research"@en .

dpv-owl:Scope a rdfs:Class,
        owl:Class ;
    dct:contributor "Harshvardhan J. Pandit" ;
    dct:created "2022-06-15"^^xsd:date ;
    rdfs:isDefinedBy dpv-owl: ;
    rdfs:subClassOf dpv-owl:Context ;
    sw:term_status "accepted"@en ;
    skos:definition "Indication of the extent or range or boundaries associated with(in) a context"@en ;
    skos:prefLabel "Scope"@en .

dpv-owl:ScoringOfIndividuals a rdfs:Class,
        owl:Class,
        dpv-owl:EvaluationScoring ;
    dct:contributor "Harshvardhan J. Pandit" ;
    dct:created "2022-10-22"^^xsd:date ;
    dct:modified "2022-11-30"^^xsd:date ;
    dct:source [ a schema:WebPage ;
            schema:name "GDPR Art.4-2" ;
            schema:url "https://eur-lex.europa.eu/eli/reg/2016/679/art_4/par_2/oj" ] ;
    rdfs:isDefinedBy dpv-owl: ;
    rdfs:subClassOf dpv-owl:EvaluationScoring ;
    sw:term_status "accepted"@en ;
    skos:definition "Processing that involves scoring of individuals"@en ;
    skos:prefLabel "Scoring of Individuals"@en .

dpv-owl:Screen a rdfs:Class,
        owl:Class,
        dpv-owl:Processing ;
    dct:contributor "Harshvardhan J. Pandit, Georg P. Krog" ;
    dct:created "2022-06-15"^^xsd:date ;
    rdfs:isDefinedBy dpv-owl: ;
    rdfs:subClassOf dpv-owl:Transform ;
    sw:term_status "accepted"@en ;
    skos:definition "to remove data for some criteria"@en ;
    skos:prefLabel "Screen"@en .

dpv-owl:Seal a rdfs:Class,
        owl:Class,
        dpv-owl:OrganisationalMeasure ;
    dct:contributor "Axel Polleres, Rob Brennan, Harshvardhan J. Pandit, Mark Lizar" ;
    dct:created "2019-04-05"^^xsd:date ;
    rdfs:isDefinedBy dpv-owl: ;
    rdfs:subClassOf dpv-owl:CertificationSeal ;
    sw:term_status "accepted"@en ;
    skos:definition "A seal or a mark indicating proof of certification to some certification or standard"@en ;
    skos:prefLabel "Seal"@en .

dpv-owl:SearchFunctionalities a rdfs:Class,
        owl:Class,
        dpv-owl:Purpose ;
    dct:contributor "Georg P. Krog" ;
    dct:created "2022-11-09"^^xsd:date ;
    rdfs:isDefinedBy dpv-owl: ;
    rdfs:subClassOf dpv-owl:ServiceProvision ;
    sw:term_status "accepted"@en ;
    skos:definition "Purposes associated with providing searching, querying, or other forms of information retrieval related functionalities"@en ;
    skos:prefLabel "Search Functionalities"@en .

dpv-owl:SecondaryImportance a rdfs:Class,
        owl:Class,
        dpv-owl:Importance ;
    dct:contributor "Harshvardhan J. Pandit, Paul Ryan, Georg P. Krog, Julian Flake, Beatriz Esteves" ;
    dct:created "2022-02-11"^^xsd:date ;
    rdfs:isDefinedBy dpv-owl: ;
    rdfs:subClassOf dpv-owl:Importance ;
    sw:term_status "accepted"@en ;
    skos:definition "Indication of 'secondary' or 'minor' or 'auxiliary' importance"@en ;
    skos:prefLabel "Secondary Importance"@en .

dpv-owl:SecretSharingSchemes a rdfs:Class,
        owl:Class,
        dpv-owl:TechnicalMeasure ;
    dct:contributor "Harshvardhan J. Pandit" ;
    dct:created "2022-08-17"^^xsd:date ;
    dct:source [ a schema:WebPage ;
            schema:name "ENISA Data Pseudonymisation: Advanced Techniques and Use Cases" ;
            schema:url "https://www.enisa.europa.eu/publications/data-pseudonymisation-advanced-techniques-and-use-cases" ] ;
    rdfs:isDefinedBy dpv-owl: ;
    rdfs:subClassOf dpv-owl:CryptographicMethods ;
    sw:term_status "accepted"@en ;
    skos:definition "Use of secret sharing schemes where the secret can only be reconstructed through combination of sufficient number of individuals"@en ;
    skos:prefLabel "Secret Sharing Schemes"@en .

dpv-owl:Sector a rdfs:Class,
        owl:Class ;
    dct:contributor "Harshvardhan J. Pandit, Javier Fernández, Axel Polleres, Elmar Kiesling, Fajar Ekaputra, Simon Steyskal" ;
    dct:created "2019-04-05"^^xsd:date ;
    vann:example dex-owl:E0043 ;
    rdfs:isDefinedBy dpv-owl: ;
    sw:term_status "accepted"@en ;
    skos:definition "Sector describes the area of application or domain that indicates or restricts scope for interpretation and application of purpose e.g. Agriculture, Banking"@en ;
    skos:prefLabel "Sector"@en ;
    skos:scopeNote "There are various sector codes used commonly to indicate the domain of an organisation or business. Examples include NACE (EU), ISIC (UN), SIC and NAICS (USA)."@en .

dpv-owl:SecureMultiPartyComputation a rdfs:Class,
        owl:Class,
        dpv-owl:TechnicalMeasure ;
    dct:contributor "Harshvardhan J. Pandit" ;
    dct:created "2022-08-17"^^xsd:date ;
    dct:source [ a schema:WebPage ;
            schema:name "ENISA Reference Incident Classification Taxonomy 2018" ;
            schema:url "https://www.enisa.europa.eu/publications/reference-incident-classification-taxonomy/" ] ;
    rdfs:isDefinedBy dpv-owl: ;
    rdfs:subClassOf dpv-owl:CryptographicMethods ;
    sw:term_status "accepted"@en ;
    skos:definition "Use of cryptographic methods for entities to jointly compute functions without revealing inputs"@en ;
    skos:prefLabel "Secure Multi-Party Computation"@en .

dpv-owl:SecureProcessingEnvironment a rdfs:Class,
        owl:Class,
        dpv-owl:OrganisationalMeasure ;
    dct:contributor "Beatriz Esteves, Harshvardhan J. Pandit" ;
    dct:created "2024-04-14"^^xsd:date ;
    dct:source "DGA 2.20"@en ;
    rdfs:isDefinedBy dpv-owl: ;
    rdfs:subClassOf dpv-owl:SecurityProcedure ;
    sw:term_status "accepted"@en ;
    skos:definition "A physical or virtual environment supported by organisational means that integrates security and compliance requirements and allows supervising data processing actions"@en ;
    skos:prefLabel "Secure Processing Environment"@en .

dpv-owl:SecurityAssessment a rdfs:Class,
        owl:Class,
        dpv-owl:OrganisationalMeasure ;
    dct:contributor "Harshvardhan J. Pandit" ;
    dct:created "2022-08-17"^^xsd:date ;
    dct:source [ a schema:WebPage ;
            schema:name "ENISA 5G Cybersecurity Standards" ;
            schema:url "https://www.enisa.europa.eu/publications/5g-cybersecurity-standards" ] ;
    rdfs:isDefinedBy dpv-owl: ;
    rdfs:subClassOf dpv-owl:RiskAssessment ;
    sw:term_status "accepted"@en ;
    skos:definition "Assessment of security intended to identity gaps, vulnerabilities, risks, and effectiveness of controls"@en ;
    skos:prefLabel "Security Assessment"@en .

dpv-owl:SecurityIncidentNotice a rdfs:Class,
        owl:Class,
        dpv-owl:OrganisationalMeasure ;
    dct:contributor "Harshvardhan J. Pandit" ;
    dct:created "2024-04-14"^^xsd:date ;
    rdfs:isDefinedBy dpv-owl: ;
    rdfs:subClassOf dpv-owl:Notice ;
    sw:term_status "accepted"@en ;
    skos:definition "A notice providing information about security incident(s)"@en ;
    skos:prefLabel "Security Incident Notice"@en .

dpv-owl:SecurityIncidentNotification a rdfs:Class,
        owl:Class,
        dpv-owl:OrganisationalMeasure ;
    dct:contributor "Harshvardhan J. Pandit" ;
    dct:created "2024-04-14"^^xsd:date ;
    rdfs:isDefinedBy dpv-owl: ;
    rdfs:subClassOf dpv-owl:Notification ;
    sw:term_status "accepted"@en ;
    skos:definition "Notification of information about security incident(s)"@en ;
    skos:prefLabel "Security Incident Notification"@en .

dpv-owl:SecurityIncidentRecord a rdfs:Class,
        owl:Class,
        dpv-owl:OrganisationalMeasure ;
    dct:contributor "Harshvardhan J. Pandit" ;
    dct:created "2024-04-14"^^xsd:date ;
    rdfs:isDefinedBy dpv-owl: ;
    rdfs:subClassOf dpv-owl:RecordsOfActivities ;
    sw:term_status "accepted"@en ;
    skos:definition "Record of a security incident"@en ;
    skos:prefLabel "Security Incident Record"@en .

dpv-owl:SecurityKnowledgeTraining a rdfs:Class,
        owl:Class,
        dpv-owl:OrganisationalMeasure ;
    dct:contributor "Harshvardhan J. Pandit" ;
    dct:created "2022-08-17"^^xsd:date ;
    dct:source [ a schema:WebPage ;
            schema:name "ENISA 5G Cybersecurity Standards" ;
            schema:url "https://www.enisa.europa.eu/publications/5g-cybersecurity-standards" ] ;
    rdfs:isDefinedBy dpv-owl: ;
    rdfs:subClassOf dpv-owl:StaffTraining ;
    sw:term_status "accepted"@en ;
    skos:definition "Training intended to increase knowledge regarding security"@en ;
    skos:prefLabel "Security Knowledge Training"@en .

dpv-owl:SecurityMethod a rdfs:Class,
        owl:Class,
        dpv-owl:TechnicalMeasure ;
    dct:contributor "Harshvardhan J. Pandit" ;
    dct:created "2022-08-24"^^xsd:date ;
    rdfs:isDefinedBy dpv-owl: ;
    rdfs:subClassOf dpv-owl:TechnicalMeasure ;
    sw:term_status "accepted"@en ;
    skos:definition "Methods that relate to creating and providing security"@en ;
    skos:prefLabel "Security Method"@en .

dpv-owl:SecurityProcedure a rdfs:Class,
        owl:Class,
        dpv-owl:OrganisationalMeasure ;
    dct:contributor "Harshvardhan J. Pandit" ;
    dct:created "2022-08-24"^^xsd:date ;
    rdfs:isDefinedBy dpv-owl: ;
    rdfs:subClassOf dpv-owl:OrganisationalMeasure ;
    sw:term_status "accepted"@en ;
    skos:definition "Procedures associated with assessing, implementing, and evaluating security"@en ;
    skos:prefLabel "Security Procedure"@en .

dpv-owl:SecurityRoleProcedures a rdfs:Class,
        owl:Class,
        dpv-owl:OrganisationalMeasure ;
    dct:contributor "Harshvardhan J. Pandit" ;
    dct:created "2022-08-17"^^xsd:date ;
    dct:source [ a schema:WebPage ;
            schema:name "ENISA 5G Cybersecurity Standards" ;
            schema:url "https://www.enisa.europa.eu/publications/5g-cybersecurity-standards" ] ;
    rdfs:isDefinedBy dpv-owl: ;
    rdfs:subClassOf dpv-owl:SecurityProcedure ;
    sw:term_status "accepted"@en ;
    skos:definition "Procedures related to security roles"@en ;
    skos:prefLabel "Security Role Procedures"@en .

dpv-owl:SellDataToThirdParties a rdfs:Class,
        owl:Class,
        dpv-owl:Purpose ;
    dct:contributor "Harshvardhan J. Pandit, Javier Fernández, Axel Polleres, Elmar Kiesling, Fajar Ekaputra, Simon Steyskal" ;
    dct:created "2019-04-05"^^xsd:date ;
    rdfs:isDefinedBy dpv-owl: ;
    rdfs:subClassOf dpv-owl:SellProducts ;
    sw:term_status "accepted"@en ;
    skos:definition "Purposes associated with selling or sharing data or information to third parties"@en ;
    skos:prefLabel "Sell Data to Third Parties"@en ;
    skos:scopeNote "Sell here means exchange, submit, or provide in return for direct or indirect compensation. Was subclass of commercial interest, changed to reflect selling something"@en .

dpv-owl:SellInsightsFromData a rdfs:Class,
        owl:Class,
        dpv-owl:Purpose ;
    dct:contributor "Harshvardhan J. Pandit, Javier Fernández, Axel Polleres, Elmar Kiesling, Fajar Ekaputra, Simon Steyskal" ;
    dct:created "2019-04-05"^^xsd:date ;
    rdfs:isDefinedBy dpv-owl: ;
    rdfs:subClassOf dpv-owl:SellProducts ;
    sw:term_status "accepted"@en ;
    skos:definition "Purposes associated with selling or sharing insights obtained from analysis of data"@en ;
    skos:prefLabel "Sell Insights from Data"@en ;
    skos:scopeNote "Sell here means exchange, submit, or provide in return for direct or indirect compensation. Was subclass of commercial interest, changed to reflect selling something"@en .

dpv-owl:SellProducts a rdfs:Class,
        owl:Class,
        dpv-owl:Purpose ;
    dct:contributor "Georg P. Krog, Harshvardhan J. Pandit, Beatriz Esteves" ;
    dct:created "2021-09-08"^^xsd:date ;
    rdfs:isDefinedBy dpv-owl: ;
    rdfs:subClassOf dpv-owl:ServiceProvision ;
    sw:term_status "accepted"@en ;
    skos:definition "Purposes associated with selling products or services"@en ;
    skos:prefLabel "Sell Products"@en ;
    skos:scopeNote "Sell here means exchange, submit, or provide in return for direct or indirect compensation."@en .

dpv-owl:SellProductsToDataSubject a rdfs:Class,
        owl:Class,
        dpv-owl:Purpose ;
    dct:contributor "Harshvardhan J. Pandit, Javier Fernández, Axel Polleres, Elmar Kiesling, Fajar Ekaputra, Simon Steyskal" ;
    dct:created "2019-04-05"^^xsd:date ;
    rdfs:isDefinedBy dpv-owl: ;
    rdfs:subClassOf dpv-owl:SellProducts ;
    sw:term_status "accepted"@en ;
    skos:definition "Purposes associated with selling products or services to the user, consumer, or data subjects"@en ;
    skos:prefLabel "Sell Products to Data Subject"@en ;
    skos:scopeNote "Sell Products here refers to processing necessary to provide and complete a sale to customers. It should not be confused with providing services with a cost based on an established agreement."@en .

dpv-owl:SensitiveData a rdfs:Class,
        owl:Class ;
    dct:created "2024-02-14"^^xsd:date ;
    rdfs:isDefinedBy dpv-owl: ;
    rdfs:subClassOf dpv-owl:Data ;
    sw:term_status "accepted"@en ;
    skos:definition "Data deemed sensitive"@en ;
    skos:prefLabel "Sensitive Data"@en .

dpv-owl:SensitiveNonPersonalData a rdfs:Class,
        owl:Class ;
    dct:created "2024-02-14"^^xsd:date ;
    dct:source "DGA 30(a)"@en ;
    rdfs:isDefinedBy dpv-owl: ;
    rdfs:subClassOf dpv-owl:SensitiveData ;
    sw:term_status "accepted"@en ;
    skos:definition "Non-personal data deemed sensitive"@en ;
    skos:prefLabel "Sensitive Non Personal Data"@en .

dpv-owl:SensitivePersonalData a rdfs:Class,
        owl:Class ;
    dct:contributor "Harshvardhan J. Pandit" ;
    dct:created "2022-01-19"^^xsd:date ;
    vann:example dex-owl:E0010,
        dex-owl:E0045 ;
    rdfs:isDefinedBy dpv-owl: ;
    rdfs:subClassOf dpv-owl:PersonalData,
        dpv-owl:SensitiveData ;
    sw:term_status "accepted"@en ;
    skos:definition "Personal data that is considered 'sensitive' in terms of privacy and/or impact, and therefore requires additional considerations and/or protection"@en ;
    skos:prefLabel "Sensitive Personal Data"@en ;
    skos:scopeNote "Sensitivity' is a matter of context, and may be defined within legal frameworks. For GDPR, Special categories of personal data are considered a subset of sensitive data. To illustrate the difference between the two, consider the situation where Location data is collected, and which is considered 'sensitive' but not 'special'. As a probable rule, sensitive data require additional considerations whereas special category data requires additional legal basis / justifications."@en .

dpv-owl:SensitivityLevel a rdfs:Class,
        owl:Class ;
    dct:contributor "Harshvardhan J. Pandit" ;
    dct:created "2023-08-24"^^xsd:date ;
    rdfs:isDefinedBy dpv-owl: ;
    rdfs:subClassOf dpv-owl:Severity ;
    sw:term_status "accepted"@en ;
    skos:definition "Sensitivity' reflects the risk of impact if not secured or utilised with appropriate measures and controls e.g. for sensitive data"@en ;
    skos:prefLabel "Sensitivity Level"@en ;
    skos:scopeNote "ISO/IEC TS 38505-3:2021 defines 'data sensitivity' as the potential harm of unauthorised disclosure. DPV's use of the concept goes beyond disclosure as it refers to the level of safeguards or controls the data requires as a reflection of its 'sensitive' nature. To indicate quantified levels of sensitivity, e.g. \"high sensitivity\", instances of severity can be directly used or specialised"@en .

dpv-owl:Service a rdfs:Class,
        owl:Class ;
    dct:contributor "Harshvardhan J. Pandit" ;
    dct:created "2024-05-09"^^xsd:date ;
    vann:example dex-owl:E0031,
        dex-owl:E0041 ;
    rdfs:isDefinedBy dpv-owl: ;
    rdfs:subClassOf dpv-owl:Process ;
    sw:term_status "accepted"@en ;
    skos:definition "A service is a process where one entity provides some benefit or assistance to another entity"@en ;
    skos:prefLabel "Service"@en ;
    skos:scopeNote "Service Provider and Service Consumer reflect the roles associated with a service. 'Service' as a process is a distinct concept from the use of 'service' as a provision method in Tech extension"@en .

dpv-owl:ServiceConsumer a rdfs:Class,
        owl:Class ;
    dct:contributor "Harshvardhan J. Pandit" ;
    dct:created "2024-04-20"^^xsd:date ;
    rdfs:isDefinedBy dpv-owl: ;
    rdfs:subClassOf dpv-owl:LegalEntity ;
    sw:term_status "accepted"@en ;
    skos:definition "The entity that consumes or receives the service"@en ;
    skos:prefLabel "Service Consumer"@en .

dpv-owl:ServiceOptimisation a rdfs:Class,
        owl:Class,
        dpv-owl:Purpose ;
    dct:contributor "Harshvardhan J. Pandit, Javier Fernández, Axel Polleres, Elmar Kiesling, Fajar Ekaputra, Simon Steyskal" ;
    dct:created "2019-04-05"^^xsd:date ;
    rdfs:isDefinedBy dpv-owl: ;
    rdfs:subClassOf dpv-owl:ServiceProvision ;
    sw:term_status "accepted"@en ;
    skos:definition "Purposes associated with optimisation of services or activities"@en ;
    skos:prefLabel "Service Optimisation"@en ;
    skos:scopeNote "Subclass of ServiceProvision since optimisation is usually considered part of providing services"@en .

dpv-owl:ServicePersonalisation a rdfs:Class,
        owl:Class,
        dpv-owl:Purpose ;
    dct:contributor "Harshvardhan J. Pandit, Javier Fernández, Axel Polleres, Elmar Kiesling, Fajar Ekaputra, Simon Steyskal" ;
    dct:created "2019-04-05"^^xsd:date ;
    rdfs:isDefinedBy dpv-owl: ;
    rdfs:subClassOf dpv-owl:Personalisation,
        dpv-owl:ServiceProvision ;
    sw:term_status "accepted"@en ;
    skos:definition "Purposes associated with providing personalisation within services or product or activities"@en ;
    skos:prefLabel "Service Personalisation"@en .

dpv-owl:ServiceProvider a rdfs:Class,
        owl:Class ;
    dct:contributor "Harshvardhan J. Pandit" ;
    dct:created "2024-04-20"^^xsd:date ;
    rdfs:isDefinedBy dpv-owl: ;
    rdfs:subClassOf dpv-owl:LegalEntity ;
    sw:term_status "accepted"@en ;
    skos:definition "The entity that provides a service"@en ;
    skos:prefLabel "Service Provider"@en .

dpv-owl:ServiceProvision a rdfs:Class,
        owl:Class,
        dpv-owl:Purpose ;
    dct:contributor "Harshvardhan J. Pandit, Javier Fernández, Axel Polleres, Elmar Kiesling, Fajar Ekaputra, Simon Steyskal" ;
    dct:created "2019-04-05"^^xsd:date ;
    rdfs:isDefinedBy dpv-owl: ;
    rdfs:subClassOf dpv-owl:Purpose ;
    sw:term_status "accepted"@en ;
    skos:definition "Purposes associated with providing service or product or activities"@en ;
    skos:prefLabel "Service Provision"@en .

dpv-owl:ServiceRegistration a rdfs:Class,
        owl:Class,
        dpv-owl:Purpose ;
    dct:contributor "Georg P. Krog, Harshvardhan J. Pandit, Beatriz Esteves" ;
    dct:created "2020-11-04"^^xsd:date ;
    rdfs:isDefinedBy dpv-owl: ;
    rdfs:subClassOf dpv-owl:ServiceProvision ;
    sw:term_status "accepted"@en ;
    skos:definition "Purposes associated with registering users and collecting information required for providing a service"@en ;
    skos:prefLabel "Service Registration"@en ;
    skos:scopeNote "An example of service registration is to provide a form that collects information such as preferred language or media format for downloading a movie"@en .

dpv-owl:ServiceUsageAnalytics a rdfs:Class,
        owl:Class,
        dpv-owl:Purpose ;
    dct:contributor "Georg P. Krog, Harshvardhan J. Pandit, Beatriz Esteves" ;
    dct:created "2020-11-04"^^xsd:date ;
    dct:modified "2022-10-05"^^xsd:date ;
    rdfs:isDefinedBy dpv-owl: ;
    rdfs:subClassOf dpv-owl:ServiceProvision ;
    sw:term_status "accepted"@en ;
    skos:definition "Purposes associated with conducting analysis and reporting related to usage of services or products"@en ;
    skos:prefLabel "Service Usage Analytics"@en ;
    skos:scopeNote "Was \"UsageAnalytics\", prefixed with Service to better reflect scope"@en .

dpv-owl:Severity a rdfs:Class,
        owl:Class ;
    dct:contributor "Harshvardhan J. Pandit" ;
    dct:created "2022-07-21"^^xsd:date ;
    vann:example dex-owl:E0068 ;
    rdfs:isDefinedBy dpv-owl: ;
    sw:term_status "accepted"@en ;
    skos:definition "The magnitude of being unwanted or having negative effects such as harmful impacts"@en ;
    skos:prefLabel "Severity"@en ;
    skos:scopeNote "Severity can be associated with Risk, or its Consequences and Impacts"@en .

dpv-owl:Share a rdfs:Class,
        owl:Class,
        dpv-owl:Processing ;
    dct:created "2019-05-07"^^xsd:date ;
    dct:source [ a schema:WebPage ;
            schema:name "GDPR Art.4-2" ;
            schema:url "https://eur-lex.europa.eu/eli/reg/2016/679/art_4/par_2/oj" ] ;
    rdfs:isDefinedBy dpv-owl: ;
    rdfs:subClassOf dpv-owl:Disclose ;
    sw:term_status "accepted"@en ;
    skos:definition "to give data (or a portion of it) to others"@en ;
    skos:prefLabel "Share"@en .

dpv-owl:SingleSignOn a rdfs:Class,
        owl:Class,
        dpv-owl:TechnicalMeasure ;
    dct:contributor "Georg P. Krog, Harshvardhan J. Pandit, Paul Ryan" ;
    dct:created "2020-11-04"^^xsd:date ;
    rdfs:isDefinedBy dpv-owl: ;
    rdfs:subClassOf dpv-owl:AuthenticationProtocols ;
    sw:term_status "accepted"@en ;
    skos:definition "Use of credentials or processes that enable using one set of credentials to authenticate multiple contexts."@en ;
    skos:prefLabel "Single Sign On"@en .

dpv-owl:SingularDataVolume a rdfs:Class,
        owl:Class,
        dpv-owl:DataVolume ;
    dct:contributor "Harshvardhan J. Pandit" ;
    dct:created "2022-06-15"^^xsd:date ;
    rdfs:isDefinedBy dpv-owl: ;
    rdfs:subClassOf dpv-owl:DataVolume ;
    sw:term_status "accepted"@en ;
    skos:definition "Data volume that is considered singular i.e. a specific instance or single item"@en ;
    skos:prefLabel "Singular Data Volume"@en .

dpv-owl:SingularFrequency a rdfs:Class,
        owl:Class,
        dpv-owl:Frequency ;
    dct:contributor "Harshvardhan J. Pandit" ;
    dct:created "2022-06-15"^^xsd:date ;
    dct:modified "2020-10-05"^^xsd:date ;
    rdfs:isDefinedBy dpv-owl: ;
    rdfs:subClassOf dpv-owl:Frequency ;
    sw:term_status "accepted"@en ;
    skos:definition "Frequency where occurrences are singular i.e. they take place only once"@en ;
    skos:prefLabel "Singular Frequency"@en .

dpv-owl:SingularScaleOfDataSubjects a rdfs:Class,
        owl:Class,
        dpv-owl:DataSubjectScale ;
    dct:contributor "Harshvardhan J. Pandit" ;
    dct:created "2022-06-15"^^xsd:date ;
    rdfs:isDefinedBy dpv-owl: ;
    rdfs:subClassOf dpv-owl:DataSubjectScale ;
    sw:term_status "accepted"@en ;
    skos:definition "Scale of data subjects considered singular i.e. a specific data subject"@en ;
    skos:prefLabel "Singular Scale Of Data Subjects"@en .

dpv-owl:SmallDataVolume a rdfs:Class,
        owl:Class,
        dpv-owl:DataVolume ;
    dct:contributor "Harshvardhan J. Pandit" ;
    dct:created "2022-06-15"^^xsd:date ;
    rdfs:isDefinedBy dpv-owl: ;
    rdfs:subClassOf dpv-owl:DataVolume ;
    sw:term_status "accepted"@en ;
    skos:definition "Data volume that is considered small or limited within the context"@en ;
    skos:prefLabel "Small Data Volume"@en .

dpv-owl:SmallScaleOfDataSubjects a rdfs:Class,
        owl:Class,
        dpv-owl:DataSubjectScale ;
    dct:contributor "Harshvardhan J. Pandit" ;
    dct:created "2022-06-15"^^xsd:date ;
    rdfs:isDefinedBy dpv-owl: ;
    rdfs:subClassOf dpv-owl:DataSubjectScale ;
    sw:term_status "accepted"@en ;
    skos:definition "Scale of data subjects considered small or limited within the context"@en ;
    skos:prefLabel "Small Scale Of Data Subjects"@en .

dpv-owl:SmallScaleProcessing a rdfs:Class,
        owl:Class,
        dpv-owl:ProcessingScale ;
    dct:contributor "Harshvardhan J. Pandit" ;
    dct:created "2022-09-07"^^xsd:date ;
    rdfs:isDefinedBy dpv-owl: ;
    rdfs:subClassOf dpv-owl:ProcessingScale ;
    sw:term_status "accepted"@en ;
    skos:definition "Processing that takes place at small scales (as specified by some criteria)"@en ;
    skos:prefLabel "Small Scale Processing"@en .

dpv-owl:SocialMediaMarketing a rdfs:Class,
        owl:Class,
        dpv-owl:Purpose ;
    dct:contributor "Georg P. Krog, Harshvardhan J. Pandit, Beatriz Esteves" ;
    dct:created "2020-11-04"^^xsd:date ;
    rdfs:isDefinedBy dpv-owl: ;
    rdfs:subClassOf dpv-owl:Marketing ;
    sw:term_status "accepted"@en ;
    skos:definition "Purposes associated with conducting marketing through social media"@en ;
    skos:prefLabel "Social Media Marketing"@en .

dpv-owl:SpecialCategoryPersonalData a rdfs:Class,
        owl:Class ;
    dct:contributor "Elmar Kiesling; Harshvardhan J. Pandit, Fajar Ekaputra" ;
    dct:created "2019-05-07"^^xsd:date ;
    dct:modified "2022-01-19"^^xsd:date ;
    dct:source [ a schema:WebPage ;
            schema:name "GDPR Art.9-1" ;
            schema:url "https://eur-lex.europa.eu/eli/reg/2016/679/art_9/par_1/oj" ] ;
    vann:example dex-owl:E0010,
        dex-owl:E0045 ;
    rdfs:isDefinedBy dpv-owl: ;
    rdfs:subClassOf dpv-owl:SensitivePersonalData ;
    sw:term_status "accepted"@en ;
    skos:definition "Sensitive Personal Data whose use requires specific additional legal permission or justification"@en ;
    skos:prefLabel "Special Category Personal Data"@en ;
    skos:scopeNote "The term 'special category' is based on GDPR Art.9, but should not be considered as exclusive to it. DPV considers all Special Categories to also be Sensitive, but whose use is either prohibited or regulated and therefore requires additional legal basis for justification that is separate from that for general personal data."@en .

dpv-owl:SporadicDataVolume a rdfs:Class,
        owl:Class,
        dpv-owl:DataVolume ;
    dct:contributor "Harshvardhan J. Pandit" ;
    dct:created "2022-06-15"^^xsd:date ;
    rdfs:isDefinedBy dpv-owl: ;
    rdfs:subClassOf dpv-owl:DataVolume ;
    sw:term_status "accepted"@en ;
    skos:definition "Data volume that is considered sporadic or sparse within the context"@en ;
    skos:prefLabel "Sporadic Data Volume"@en .

dpv-owl:SporadicFrequency a rdfs:Class,
        owl:Class,
        dpv-owl:Frequency ;
    dct:contributor "Harshvardhan J. Pandit" ;
    dct:created "2022-06-15"^^xsd:date ;
    dct:modified "2020-10-05"^^xsd:date ;
    rdfs:isDefinedBy dpv-owl: ;
    rdfs:subClassOf dpv-owl:Frequency ;
    sw:term_status "accepted"@en ;
    skos:definition "Frequency where occurrences are sporadic or infrequent or sparse"@en ;
    skos:prefLabel "Sporadic Frequency"@en .

dpv-owl:SporadicScaleOfDataSubjects a rdfs:Class,
        owl:Class,
        dpv-owl:DataSubjectScale ;
    dct:contributor "Harshvardhan J. Pandit" ;
    dct:created "2022-06-15"^^xsd:date ;
    rdfs:isDefinedBy dpv-owl: ;
    rdfs:subClassOf dpv-owl:DataSubjectScale ;
    sw:term_status "accepted"@en ;
    skos:definition "Scale of data subjects considered sporadic or sparse within the context"@en ;
    skos:prefLabel "Sporadic Scale Of Data Subjects"@en .

dpv-owl:StaffTraining a rdfs:Class,
        owl:Class,
        dpv-owl:OrganisationalMeasure ;
    dct:contributor "Axel Polleres, Rob Brennan, Harshvardhan J. Pandit, Mark Lizar" ;
    dct:created "2019-04-05"^^xsd:date ;
    vann:example dex-owl:E0021 ;
    rdfs:isDefinedBy dpv-owl: ;
    rdfs:subClassOf dpv-owl:OrganisationalMeasure ;
    sw:term_status "accepted"@en ;
    skos:definition "Practices and policies regarding training of staff members"@en ;
    skos:prefLabel "Staff Training"@en .

dpv-owl:StandardsConformance a rdfs:Class,
        owl:Class,
        dpv-owl:OrganisationalMeasure ;
    dct:contributor "Beatriz Esteves, Harshvardhan J. Pandit" ;
    dct:created "2024-04-14"^^xsd:date ;
    dct:source "DGA 12.d"@en ;
    rdfs:isDefinedBy dpv-owl: ;
    rdfs:subClassOf dpv-owl:GovernanceProcedures ;
    sw:term_status "accepted"@en ;
    skos:definition "Purposes associated with activities undertaken to ensure or achieve conformance with standards"@en ;
    skos:prefLabel "Standards Conformance"@en .

dpv-owl:StatisticalConfidentialityAgreement a rdfs:Class,
        owl:Class,
        dpv-owl:LegalMeasure ;
    dct:created "2022-02-09"^^xsd:date ;
    rdfs:isDefinedBy dpv-owl: ;
    rdfs:subClassOf dpv-owl:LegalAgreement ;
    sw:term_status "accepted"@en ;
    skos:definition "An agreement outlining conditions, criteria, obligations, responsibilities, and specifics for classification and management of 'confidential data' based on a statistical framework"@en ;
    skos:prefLabel "Statistical Confidentiality Agreement"@en .

dpv-owl:StatisticallyConfidentialData a rdfs:Class,
        owl:Class ;
    dct:created "2024-02-14"^^xsd:date ;
    dct:source "DGA 2(20)"@en ;
    rdfs:isDefinedBy dpv-owl: ;
    rdfs:subClassOf dpv-owl:ConfidentialData ;
    sw:term_status "accepted"@en ;
    skos:definition "Data protected through Statistical Confidentiality regulations and agreements"@en ;
    skos:prefLabel "Statistically Confidential Data"@en .

dpv-owl:Status a rdfs:Class,
        owl:Class ;
    dct:contributor "Harshvardhan J. Pandit" ;
    dct:created "2022-05-18"^^xsd:date ;
    rdfs:isDefinedBy dpv-owl: ;
    rdfs:subClassOf dpv-owl:Context ;
    sw:term_status "accepted"@en ;
    skos:definition "The status or state of something"@en ;
    skos:prefLabel "Status"@en .

dpv-owl:StorageCondition a rdfs:Class,
        owl:Class ;
    dct:contributor "Axel Polleres, Rob Brennan, Harshvardhan J. Pandit, Mark Lizar" ;
    dct:created "2019-04-05"^^xsd:date ;
    vann:example dex-owl:E0011,
        dex-owl:E0048 ;
    rdfs:isDefinedBy dpv-owl: ;
    rdfs:subClassOf dpv-owl:ProcessingCondition ;
    sw:term_status "accepted"@en ;
    skos:definition "Conditions required or followed regarding storage of data"@en ;
    skos:prefLabel "Storage Condition"@en .

dpv-owl:StorageDeletion a rdfs:Class,
        owl:Class ;
    dct:contributor "Axel Polleres, Rob Brennan, Harshvardhan J. Pandit, Mark Lizar" ;
    dct:created "2019-04-05"^^xsd:date ;
    vann:example dex-owl:E0048 ;
    rdfs:isDefinedBy dpv-owl: ;
    rdfs:subClassOf dpv-owl:StorageCondition ;
    sw:term_status "accepted"@en ;
    skos:definition "Deletion or Erasure of data including any deletion guarantees"@en ;
    skos:prefLabel "Storage Deletion"@en .

dpv-owl:StorageDuration a rdfs:Class,
        owl:Class ;
    dct:contributor "Axel Polleres, Rob Brennan, Harshvardhan J. Pandit, Mark Lizar" ;
    dct:created "2019-04-05"^^xsd:date ;
    vann:example dex-owl:E0048 ;
    rdfs:isDefinedBy dpv-owl: ;
    rdfs:subClassOf dpv-owl:ProcessingDuration,
        dpv-owl:StorageCondition ;
    sw:term_status "accepted"@en ;
    skos:definition "Duration or temporal limitation on storage of data"@en ;
    skos:prefLabel "Storage Duration"@en .

dpv-owl:StorageLocation a rdfs:Class,
        owl:Class ;
    dct:contributor "Axel Polleres, Rob Brennan, Harshvardhan J. Pandit, Mark Lizar" ;
    dct:created "2019-04-05"^^xsd:date ;
    vann:example dex-owl:E0048 ;
    rdfs:isDefinedBy dpv-owl: ;
    rdfs:subClassOf dpv-owl:ProcessingLocation,
        dpv-owl:StorageCondition ;
    sw:term_status "accepted"@en ;
    skos:definition "Location or geospatial scope where the data is stored"@en ;
    skos:prefLabel "Storage Location"@en .

dpv-owl:StorageRestoration a rdfs:Class,
        owl:Class ;
    dct:contributor "Axel Polleres, Rob Brennan, Harshvardhan J. Pandit, Mark Lizar" ;
    dct:created "2019-04-05"^^xsd:date ;
    vann:example dex-owl:E0048 ;
    rdfs:isDefinedBy dpv-owl: ;
    rdfs:subClassOf dpv-owl:StorageCondition ;
    sw:term_status "accepted"@en ;
    skos:definition "Regularity and temporal span of data restoration/backup mechanisms that guarantee that data is preserved"@en ;
    skos:prefLabel "Storage Restoration"@en .

dpv-owl:Store a rdfs:Class,
        owl:Class,
        dpv-owl:Processing ;
    dct:created "2019-05-07"^^xsd:date ;
    dct:source [ a schema:WebPage ;
            schema:name "GDPR Art.4-2" ;
            schema:url "https://eur-lex.europa.eu/eli/reg/2016/679/art_4/par_2/oj" ] ;
    rdfs:isDefinedBy dpv-owl: ;
    rdfs:subClassOf dpv-owl:Processing ;
    sw:term_status "accepted"@en ;
    skos:definition "to keep data for future use"@en ;
    skos:prefLabel "Store"@en .

dpv-owl:Structure a rdfs:Class,
        owl:Class,
        dpv-owl:Processing ;
    dct:created "2019-05-07"^^xsd:date ;
    dct:source [ a schema:WebPage ;
            schema:name "GDPR Art.4-2" ;
            schema:url "https://eur-lex.europa.eu/eli/reg/2016/679/art_4/par_2/oj" ] ;
    rdfs:isDefinedBy dpv-owl: ;
    rdfs:subClassOf dpv-owl:Organise ;
    sw:term_status "accepted"@en ;
    skos:definition "to arrange data according to a structure"@en ;
    skos:prefLabel "Structure"@en .

dpv-owl:Student a rdfs:Class,
        owl:Class,
        dpv-owl:DataSubject ;
    dct:contributor "Harshvardhan J. Pandit, Georg P. Krog, Julian Flake, Paul Ryan, Beatriz Esteves" ;
    dct:created "2022-04-06"^^xsd:date ;
    rdfs:isDefinedBy dpv-owl: ;
    rdfs:subClassOf dpv-owl:DataSubject ;
    sw:term_status "accepted"@en ;
    skos:definition "Data subjects that are students"@en ;
    skos:prefLabel "Student"@en .

dpv-owl:SubProcessorAgreement a rdfs:Class,
        owl:Class,
        dpv-owl:LegalMeasure ;
    dct:contributor "Georg P. Krog, Harshvardhan J. Pandit, Beatriz Esteves, Paul Ryan, Julian Flake" ;
    dct:created "2022-01-26"^^xsd:date ;
    rdfs:isDefinedBy dpv-owl: ;
    rdfs:subClassOf dpv-owl:DataProcessingAgreement ;
    sw:term_status "accepted"@en ;
    skos:definition "An agreement outlining conditions, criteria, obligations, responsibilities, and specifics for carrying out processing of data between a Data Processor and a Data (Sub-)Processor"@en ;
    skos:prefLabel "Sub-Processor Agreement"@en .

dpv-owl:Subscriber a rdfs:Class,
        owl:Class,
        dpv-owl:DataSubject ;
    dct:contributor "Harshvardhan J. Pandit, Georg P. Krog, Julian Flake, Paul Ryan, Beatriz Esteves" ;
    dct:created "2022-04-06"^^xsd:date ;
    rdfs:isDefinedBy dpv-owl: ;
    rdfs:subClassOf dpv-owl:DataSubject ;
    sw:term_status "accepted"@en ;
    skos:definition "Data subjects that subscribe to service(s)"@en ;
    skos:prefLabel "Subscriber"@en ;
    skos:scopeNote "note: subscriber can be customer or consumer"@en .

dpv-owl:SubsidiaryLegalEntity a rdfs:Class,
        owl:Class ;
    dct:contributor "Harshvardhan J. Pandit, Georg P. Krog" ;
    dct:created "2024-04-14"^^xsd:date ;
    rdfs:isDefinedBy dpv-owl: ;
    rdfs:subClassOf dpv-owl:Organisation ;
    sw:term_status "accepted"@en ;
    skos:definition "A legal entity that operates as a subsidiary of another legal entity"@en ;
    skos:prefLabel "Subsidiary Legal Entity"@en .

dpv-owl:SupportContractNegotiation a rdfs:Class,
        owl:Class,
        dpv-owl:OrganisationalMeasure ;
    dct:contributor "Beatriz Esteves, Harshvardhan J. Pandit" ;
    dct:created "2024-04-14"^^xsd:date ;
    dct:source "DGA 2.15"@en ;
    rdfs:isDefinedBy dpv-owl: ;
    rdfs:subClassOf dpv-owl:SupportEntityDecisionMaking ;
    sw:term_status "accepted"@en ;
    skos:definition "Supporting entities, including individuals, with negotiating a contract and its terms and conditions"@en ;
    skos:prefLabel "Support Contract Negotiation"@en .

dpv-owl:SupportEntityDecisionMaking a rdfs:Class,
        owl:Class,
        dpv-owl:OrganisationalMeasure ;
    dct:contributor "Beatriz Esteves, Harshvardhan J. Pandit" ;
    dct:created "2024-04-14"^^xsd:date ;
    dct:source "DGA 2.15"@en ;
    rdfs:isDefinedBy dpv-owl: ;
    rdfs:subClassOf dpv-owl:OrganisationalMeasure ;
    sw:term_status "accepted"@en ;
    skos:definition "Supporting entities, including individuals, in making decisions"@en ;
    skos:prefLabel "Support Entity Decision Making"@en .

dpv-owl:SupportExchangeOfViews a rdfs:Class,
        owl:Class,
        dpv-owl:OrganisationalMeasure ;
    dct:contributor "Beatriz Esteves, Harshvardhan J. Pandit" ;
    dct:created "2024-04-14"^^xsd:date ;
    dct:source "DGA 2.15"@en ;
    rdfs:isDefinedBy dpv-owl: ;
    rdfs:subClassOf dpv-owl:SupportEntityDecisionMaking ;
    sw:term_status "accepted"@en ;
    skos:definition "Supporting individuals and entities in exchanging views e.g. regarding data processing purposes for their best interests"@en ;
    skos:prefLabel "Support Exchange of Views"@en .

dpv-owl:SupportInformedConsentDecision a rdfs:Class,
        owl:Class,
        dpv-owl:OrganisationalMeasure ;
    dct:contributor "Beatriz Esteves, Harshvardhan J. Pandit" ;
    dct:created "2024-04-14"^^xsd:date ;
    dct:source "DGA 2.15"@en ;
    rdfs:isDefinedBy dpv-owl: ;
    rdfs:subClassOf dpv-owl:SupportEntityDecisionMaking ;
    sw:term_status "accepted"@en ;
    skos:definition "Supporting individuals with making a decision regarding their informed consent"@en ;
    skos:prefLabel "Support Informed Consent Decision"@en .

dpv-owl:SupraNationalAuthority a rdfs:Class,
        owl:Class ;
    dct:contributor "Harshvardhan J. Pandit" ;
    dct:created "2022-02-02"^^xsd:date ;
    dct:source [ a schema:WebPage ;
            schema:name "ADMS controlled vocabulary" ;
            schema:url "http://purl.org/adms" ] ;
    rdfs:isDefinedBy dpv-owl: ;
    rdfs:subClassOf dpv-owl:Authority ;
    sw:term_status "accepted"@en ;
    skos:definition "An authority tasked with overseeing legal compliance for a supra-national union e.g. EU"@en ;
    skos:prefLabel "Supranational Authority"@en .

dpv-owl:SupraNationalUnion a rdfs:Class,
        owl:Class ;
    dct:contributor "Harshvardhan J. Pandit" ;
    dct:created "2022-01-19"^^xsd:date ;
    rdfs:isDefinedBy dpv-owl: ;
    rdfs:subClassOf dpv-owl:Location ;
    sw:term_status "accepted"@en ;
    skos:definition "A political union of two or more countries with an establishment of common authority"@en ;
    skos:prefLabel "Supranational Union"@en .

dpv-owl:SymmetricCryptography a rdfs:Class,
        owl:Class,
        dpv-owl:TechnicalMeasure ;
    dct:contributor "Harshvardhan J. Pandit" ;
    dct:created "2022-08-17"^^xsd:date ;
    dct:source [ a schema:WebPage ;
            schema:name "ENISA Reference Incident Classification Taxonomy 2018" ;
            schema:url "https://www.enisa.europa.eu/publications/reference-incident-classification-taxonomy/" ] ;
    rdfs:isDefinedBy dpv-owl: ;
    rdfs:subClassOf dpv-owl:CryptographicMethods ;
    sw:term_status "accepted"@en ;
    skos:definition "Use of cryptography where the same keys are utilised for encryption and decryption of information"@en ;
    skos:prefLabel "Symmetric Cryptography"@en .

dpv-owl:SymmetricEncryption a rdfs:Class,
        owl:Class,
        dpv-owl:TechnicalMeasure ;
    dct:contributor "Harshvardhan J. Pandit" ;
    dct:created "2022-08-17"^^xsd:date ;
    dct:source [ a schema:WebPage ;
            schema:name "ENISA Data Pseudonymisation: Advanced Techniques and Use Cases" ;
            schema:url "https://www.enisa.europa.eu/publications/data-pseudonymisation-advanced-techniques-and-use-cases" ] ;
    rdfs:isDefinedBy dpv-owl: ;
    rdfs:subClassOf dpv-owl:Encryption ;
    sw:term_status "accepted"@en ;
    skos:definition "Use of symmetric cryptography to encrypt data"@en ;
    skos:prefLabel "Symmetric Encryption"@en .

dpv-owl:SyntheticData a rdfs:Class,
        owl:Class ;
    dct:contributor "Harshvardhan J. Pandit" ;
    dct:created "2022-08-18"^^xsd:date ;
    dct:modified "2023-12-10"^^xsd:date ;
    dct:source [ a schema:WebPage ;
            schema:name "ENISA Data Protection Engineering" ;
            schema:url "https://www.enisa.europa.eu/publications/data-protection-engineering" ] ;
    rdfs:isDefinedBy dpv-owl: ;
    rdfs:subClassOf dpv-owl:GeneratedData ;
    sw:term_status "accepted"@en ;
    skos:definition "Synthetic data refers to artificially created data such that it is intended to resemble real data (personal or non-personal), but does not refer to any specific identified or identifiable individual, or to the real measure of an observable parameter in the case of non-personal data"@en ;
    skos:prefLabel "Synthetic Data"@en .

dpv-owl:SystematicMonitoring a rdfs:Class,
        owl:Class,
        dpv-owl:ProcessingContext ;
    dct:contributor "Harshvardhan J. Pandit, Piero Bonatti" ;
    dct:created "2020-11-04"^^xsd:date ;
    dct:source [ a schema:WebPage ;
            schema:name "GDPR Art.4-2" ;
            schema:url "https://eur-lex.europa.eu/eli/reg/2016/679/art_4/par_2/oj" ] ;
    rdfs:isDefinedBy dpv-owl: ;
    rdfs:subClassOf dpv-owl:ProcessingContext ;
    sw:term_status "accepted"@en ;
    skos:definition "Processing that involves systematic monitoring of individuals"@en ;
    skos:prefLabel "Systematic Monitoring"@en .

dpv-owl:TargetedAdvertising a rdfs:Class,
        owl:Class,
        dpv-owl:Purpose ;
    dct:contributor "Harshvardhan J. Pandit" ;
    dct:created "2022-03-30"^^xsd:date ;
    rdfs:isDefinedBy dpv-owl: ;
    rdfs:subClassOf dpv-owl:PersonalisedAdvertising ;
    sw:term_status "accepted"@en ;
    skos:definition "Purposes associated with creating and providing personalised advertisement where the personalisation is targeted to a specific individual or group of individuals"@en ;
    skos:prefLabel "Targeted Advertising"@en .

dpv-owl:TechnicalMeasure a rdfs:Class,
        owl:Class ;
    dct:contributor "Axel Polleres, Rob Brennan, Harshvardhan J. Pandit, Mark Lizar" ;
    dct:created "2019-04-05"^^xsd:date ;
    dct:modified "2023-12-10"^^xsd:date ;
    vann:example dex-owl:E0020,
        dex-owl:E0064 ;
    rdfs:isDefinedBy dpv-owl: ;
    rdfs:subClassOf dpv-owl:TechnicalOrganisationalMeasure ;
    sw:term_status "accepted"@en ;
    skos:definition "Technical measures used to safeguard and ensure good practices in connection with data and technologies"@en ;
    skos:prefLabel "Technical Measure"@en .

dpv-owl:TechnicalOrganisationalMeasure a rdfs:Class,
        owl:Class ;
    dct:contributor "Bud Bruegger" ;
    dct:created "2019-04-05"^^xsd:date ;
    dct:modified "2023-12-10"^^xsd:date ;
    rdfs:isDefinedBy dpv-owl: ;
    sw:term_status "accepted"@en ;
    skos:definition "Technical and Organisational measures used to safeguard and ensure good practices in connection with data and technologies"@en ;
    skos:prefLabel "Technical and Organisational Measure"@en .

dpv-owl:TechnicalServiceProvision a rdfs:Class,
        owl:Class,
        dpv-owl:Purpose ;
    dct:contributor "Harshvardhan J. Pandit" ;
    dct:created "2021-09-08"^^xsd:date ;
    rdfs:isDefinedBy dpv-owl: ;
    rdfs:subClassOf dpv-owl:ServiceProvision ;
    sw:term_status "accepted"@en ;
    skos:definition "Purposes associated with managing and providing technical processes and functions necessary for delivering services"@en ;
    skos:prefLabel "Technical Service Provision"@en .

dpv-owl:Technology a rdfs:Class,
        owl:Class ;
    dct:contributor "Harshvardhan J. Pandit" ;
    dct:created "2022-01-26"^^xsd:date ;
    rdfs:isDefinedBy dpv-owl: ;
    sw:term_status "accepted"@en ;
    skos:definition "The technology, technological implementation, or any techniques, skills, methods, and processes used or applied"@en ;
    skos:prefLabel "Technology"@en ;
    skos:scopeNote "Examples (non-exhaustive) include: Algorithm, Process, Method, Skill, Database, Cookies, Server, Device"@en .

dpv-owl:TemporalDuration a rdfs:Class,
        owl:Class ;
    dct:contributor "Harshvardhan J. Pandit" ;
    dct:created "2022-06-15"^^xsd:date ;
    dct:modified "2020-10-05"^^xsd:date ;
    rdfs:isDefinedBy dpv-owl: ;
    rdfs:subClassOf dpv-owl:Duration ;
    sw:term_status "accepted"@en ;
    skos:definition "Duration that has a fixed temporal duration e.g. 6 months"@en ;
    skos:prefLabel "Temporal Duration"@en .

dpv-owl:ThirdCountry a rdfs:Class,
        owl:Class ;
    dct:contributor "Harshvardhan J. Pandit" ;
    dct:created "2022-02-09"^^xsd:date ;
    rdfs:isDefinedBy dpv-owl: ;
    rdfs:subClassOf dpv-owl:Country ;
    sw:term_status "accepted"@en ;
    skos:definition "Represents a country outside applicable or compatible jurisdiction as outlined in law"@en ;
    skos:prefLabel "Third Country"@en .

dpv-owl:ThirdParty a rdfs:Class,
        owl:Class ;
    dct:contributor "Harshvardhan J. Pandit" ;
    dct:created "2019-06-04"^^xsd:date ;
    dct:modified "2024-05-21"^^xsd:date ;
    dct:source [ a schema:WebPage ;
            schema:name "GDPR Art.4-10" ;
            schema:url "https://eur-lex.europa.eu/eli/reg/2016/679/art_4/par_10/oj" ] ;
    rdfs:isDefinedBy dpv-owl: ;
    rdfs:subClassOf dpv-owl:Recipient ;
    sw:term_status "accepted"@en ;
    skos:definition "A ‘third party’ means any natural or legal person other than - the entities directly involved or operating under those directly involved in a process"@en ;
    skos:prefLabel "Third Party"@en ;
    skos:scopeNote "Third Party in the context of personal data processing are entities other than the data subject, controllers, processors, and authorities"@en .

dpv-owl:ThirdPartyAgreement a rdfs:Class,
        owl:Class,
        dpv-owl:LegalMeasure ;
    dct:contributor "Harshvardhan J. Pandit" ;
    dct:created "2022-02-09"^^xsd:date ;
    rdfs:isDefinedBy dpv-owl: ;
    rdfs:subClassOf dpv-owl:DataProcessingAgreement ;
    sw:term_status "accepted"@en ;
    skos:definition "An agreement outlining conditions, criteria, obligations, responsibilities, and specifics for carrying out processing of data between a Data Controller or Processor and a Third Party"@en ;
    skos:prefLabel "Third-Party Agreement"@en .

dpv-owl:ThirdPartyContract a rdfs:Class,
        owl:Class,
        dpv-owl:LegalBasis ;
    dct:created "2023-12-10"^^xsd:date ;
    rdfs:isDefinedBy dpv-owl: ;
    rdfs:subClassOf dpv-owl:Contract ;
    sw:term_status "accepted"@en ;
    skos:definition "Creation, completion, fulfilment, or performance of a contract, with the Data Controller and Third Party as parties, and involving specified processing of data or technologies"@en ;
    skos:prefLabel "Third Party Contract"@en .

dpv-owl:ThirdPartyDataSource a rdfs:Class,
        owl:Class,
        dpv-owl:DataSource ;
    dct:created "2023-10-12"^^xsd:date ;
    rdfs:isDefinedBy dpv-owl: ;
    rdfs:subClassOf dpv-owl:DataSource ;
    sw:term_status "accepted"@en ;
    skos:definition "Data Sourced from a Third Party, e.g. when data is collected from an entity that is neither the Controller nor the Data Subject"@en ;
    skos:prefLabel "Third Party as Data Source"@en .

dpv-owl:ThirdPartySecurityProcedures a rdfs:Class,
        owl:Class,
        dpv-owl:OrganisationalMeasure ;
    dct:contributor "Harshvardhan J. Pandit" ;
    dct:created "2022-08-17"^^xsd:date ;
    dct:source [ a schema:WebPage ;
            schema:name "ENISA 5G Cybersecurity Standards" ;
            schema:url "https://www.enisa.europa.eu/publications/5g-cybersecurity-standards" ] ;
    rdfs:isDefinedBy dpv-owl: ;
    rdfs:subClassOf dpv-owl:SecurityProcedure ;
    sw:term_status "accepted"@en ;
    skos:definition "Procedures related to security associated with Third Parties"@en ;
    skos:prefLabel "Third Party Security Procedures"@en .

dpv-owl:Tourist a rdfs:Class,
        owl:Class,
        dpv-owl:DataSubject ;
    dct:contributor "Harshvardhan J. Pandit, Georg P. Krog, Julian Flake, Paul Ryan, Beatriz Esteves" ;
    dct:created "2022-04-06"^^xsd:date ;
    rdfs:isDefinedBy dpv-owl: ;
    rdfs:subClassOf dpv-owl:DataSubject ;
    sw:term_status "accepted"@en ;
    skos:definition "Data subjects that are tourists i.e. not citizens and not immigrants"@en ;
    skos:prefLabel "Tourist"@en .

dpv-owl:Transfer a rdfs:Class,
        owl:Class,
        dpv-owl:Processing ;
    dct:created "2019-05-07"^^xsd:date ;
    dct:source [ a schema:WebPage ;
            schema:name "SPECIAL Project" ;
            schema:url "https://specialprivacy.ercim.eu/vocabs/processing" ] ;
    vann:example dex-owl:E0035 ;
    rdfs:isDefinedBy dpv-owl: ;
    rdfs:subClassOf dpv-owl:Processing ;
    sw:term_status "accepted"@en ;
    skos:definition "to move data from one place to another"@en ;
    skos:prefLabel "Transfer"@en ;
    skos:related svpr:Transfer .

dpv-owl:Transform a rdfs:Class,
        owl:Class,
        dpv-owl:Processing ;
    dct:created "2019-05-07"^^xsd:date ;
    dct:source [ a schema:WebPage ;
            schema:name "GDPR Art.4-2" ;
            schema:url "https://eur-lex.europa.eu/eli/reg/2016/679/art_4/par_2/oj" ] ;
    rdfs:isDefinedBy dpv-owl: ;
    rdfs:subClassOf dpv-owl:Processing ;
    sw:term_status "accepted"@en ;
    skos:definition "to change the form or nature of data"@en ;
    skos:prefLabel "Transform"@en .

dpv-owl:Transmit a rdfs:Class,
        owl:Class,
        dpv-owl:Processing ;
    dct:created "2019-05-07"^^xsd:date ;
    dct:source [ a schema:WebPage ;
            schema:name "GDPR Art.4-2" ;
            schema:url "https://eur-lex.europa.eu/eli/reg/2016/679/art_4/par_2/oj" ] ;
    rdfs:isDefinedBy dpv-owl: ;
    rdfs:subClassOf dpv-owl:Disclose ;
    sw:term_status "accepted"@en ;
    skos:definition "to send out data"@en ;
    skos:prefLabel "Transmit"@en .

dpv-owl:TrustedComputing a rdfs:Class,
        owl:Class,
        dpv-owl:TechnicalMeasure ;
    dct:contributor "Harshvardhan J. Pandit" ;
    dct:created "2022-08-17"^^xsd:date ;
    dct:source [ a schema:WebPage ;
            schema:name "ENISA Reference Incident Classification Taxonomy 2018" ;
            schema:url "https://www.enisa.europa.eu/publications/reference-incident-classification-taxonomy/" ] ;
    rdfs:isDefinedBy dpv-owl: ;
    rdfs:subClassOf dpv-owl:CryptographicMethods ;
    sw:term_status "accepted"@en ;
    skos:definition "Use of cryptographic methods to restrict access and execution to trusted parties and code"@en ;
    skos:prefLabel "Trusted Computing"@en .

dpv-owl:TrustedExecutionEnvironment a rdfs:Class,
        owl:Class,
        dpv-owl:TechnicalMeasure ;
    dct:contributor "Harshvardhan J. Pandit" ;
    dct:created "2022-08-17"^^xsd:date ;
    dct:modified "2024-04-14"^^xsd:date ;
    dct:source [ a schema:WebPage ;
            schema:name "ENISA Data Protection Engineering" ;
            schema:url "https://www.enisa.europa.eu/publications/data-protection-engineering" ] ;
    rdfs:isDefinedBy dpv-owl: ;
    rdfs:subClassOf dpv-owl:CryptographicMethods ;
    sw:term_status "accepted"@en ;
    skos:definition "Use of cryptographic methods to restrict access and execution to trusted parties and code within a dedicated execution environment"@en ;
    skos:prefLabel "Trusted Execution Environment"@en .

dpv-owl:Unexpected a rdfs:Class,
        owl:Class,
        dpv-owl:ExpectationStatus ;
    dct:contributor "Harshvardhan J. Pandit, Delaram Golpayegani, Georg P. Krog, Paul Ryan" ;
    dct:created "2024-05-10"^^xsd:date ;
    rdfs:isDefinedBy dpv-owl: ;
    rdfs:subClassOf dpv-owl:ExpectationStatus ;
    sw:term_status "accepted"@en ;
    skos:definition "Status indicating the specified context was unexpected i.e. not expected"@en ;
    skos:prefLabel "Unexpected"@en .

dpv-owl:UninformedConsent a rdfs:Class,
        owl:Class,
        dpv-owl:LegalBasis ;
    dct:contributor "Georg P. Krog, Harshvardhan J. Pandit, Paul Ryan, Julian Flake" ;
    dct:created "2022-06-21"^^xsd:date ;
    rdfs:isDefinedBy dpv-owl: ;
    rdfs:subClassOf dpv-owl:Consent ;
    sw:term_status "accepted"@en ;
    skos:definition "Consent that is uninformed i.e. without requirement to provide sufficient information to make a consenting decision"@en ;
    skos:prefLabel "Uninformed Consent"@en .

dpv-owl:Unintended a rdfs:Class,
        owl:Class,
        dpv-owl:IntentionStatus ;
    dct:contributor "Harshvardhan J. Pandit, Delaram Golpayegani, Georg P. Krog, Paul Ryan" ;
    dct:created "2024-05-10"^^xsd:date ;
    rdfs:isDefinedBy dpv-owl: ;
    rdfs:subClassOf dpv-owl:IntentionStatus ;
    sw:term_status "accepted"@en ;
    skos:definition "Status indicating the specified context was unintended i.e. not intended"@en ;
    skos:prefLabel "Unintended"@en .

dpv-owl:UnknownApplicability a rdfs:Class,
        owl:Class,
        dpv-owl:Applicability ;
    dct:contributor "Harshvardhan J. Pandit" ;
    dct:created "2023-08-24"^^xsd:date ;
    rdfs:isDefinedBy dpv-owl: ;
    rdfs:subClassOf dpv-owl:Applicability ;
    sw:term_status "accepted"@en ;
    skos:definition "Concept indicating information or context availability is unknown i.e. it is not known if the information exists or is applicable and therefore statements about its availability cannot be made (yet)"@en ;
    skos:prefLabel "Unknown Applicability"@en ;
    skos:scopeNote "This concept is useful when describing situations where it cannot be stated whether the context applies or whether the information is not available yet. For example, if a form field asks about whether a process X was completed and it is not yet known whether X applies or not and therefore it is also unclear whether X was completed or not. Using UnknownApplicability is a signal that the applicability of X should be assessed, and if applicable, then information about X should be identified and used here."@en .

dpv-owl:Unlawful a rdfs:Class,
        owl:Class,
        dpv-owl:Lawfulness ;
    dct:contributor "Harshvardhan J. Pandit" ;
    dct:created "2022-10-19"^^xsd:date ;
    rdfs:isDefinedBy dpv-owl: ;
    rdfs:subClassOf dpv-owl:Lawfulness ;
    sw:term_status "accepted"@en ;
    skos:definition "State of being unlawful or legally non-compliant"@en ;
    skos:prefLabel "Unlawful"@en .

dpv-owl:UntilEventDuration a rdfs:Class,
        owl:Class ;
    dct:contributor "Harshvardhan J. Pandit" ;
    dct:created "2022-06-15"^^xsd:date ;
    dct:modified "2020-10-05"^^xsd:date ;
    rdfs:isDefinedBy dpv-owl: ;
    rdfs:subClassOf dpv-owl:Duration ;
    sw:term_status "accepted"@en ;
    skos:definition "Duration that takes place until a specific event occurs e.g. Account Closure"@en ;
    skos:prefLabel "Until Event Duration"@en .

dpv-owl:UntilTimeDuration a rdfs:Class,
        owl:Class ;
    dct:contributor "Harshvardhan J. Pandit" ;
    dct:created "2022-06-15"^^xsd:date ;
    dct:modified "2020-10-05"^^xsd:date ;
    rdfs:isDefinedBy dpv-owl: ;
    rdfs:subClassOf dpv-owl:Duration ;
    sw:term_status "accepted"@en ;
    skos:definition "Duration that has a fixed end date e.g. 2022-12-31"@en ;
    skos:prefLabel "Until Time Duration"@en .

dpv-owl:UnverifiedData a rdfs:Class,
        owl:Class ;
    dct:contributor "Harshvardhan J. Pandit" ;
    dct:created "2022-11-02"^^xsd:date ;
    rdfs:isDefinedBy dpv-owl: ;
    rdfs:subClassOf dpv-owl:Data ;
    sw:term_status "accepted"@en ;
    skos:definition "Data that has not been verified in terms of accuracy, inconsistency, or quality"@en ;
    skos:prefLabel "Unverified Data"@en .

dpv-owl:UsageControl a rdfs:Class,
        owl:Class,
        dpv-owl:TechnicalMeasure ;
    dct:contributor "Harshvardhan J. Pandit" ;
    dct:created "2022-08-17"^^xsd:date ;
    dct:source [ a schema:WebPage ;
            schema:name "ENISA Reference Incident Classification Taxonomy 2018" ;
            schema:url "https://www.enisa.europa.eu/publications/reference-incident-classification-taxonomy/" ] ;
    rdfs:isDefinedBy dpv-owl: ;
    rdfs:subClassOf dpv-owl:AccessControlMethod ;
    sw:term_status "accepted"@en ;
    skos:definition "Management of usage, which is intended to be broader than access control and may cover trust, digital rights, or other relevant controls"@en ;
    skos:prefLabel "Usage Control"@en .

dpv-owl:Use a rdfs:Class,
        owl:Class,
        dpv-owl:Processing ;
    dct:created "2019-05-07"^^xsd:date ;
    dct:source [ a schema:WebPage ;
            schema:name "GDPR Art.4-2" ;
            schema:url "https://eur-lex.europa.eu/eli/reg/2016/679/art_4/par_2/oj" ] ;
    rdfs:isDefinedBy dpv-owl: ;
    rdfs:subClassOf dpv-owl:Processing ;
    sw:term_status "accepted"@en ;
    skos:definition "to use data"@en ;
    skos:prefLabel "Use"@en .

dpv-owl:UseSyntheticData a rdfs:Class,
        owl:Class,
        dpv-owl:TechnicalMeasure ;
    dct:contributor "Harshvardhan J. Pandit" ;
    dct:created "2022-08-17"^^xsd:date ;
    dct:source [ a schema:WebPage ;
            schema:name "ENISA Data Protection Engineering" ;
            schema:url "https://www.enisa.europa.eu/publications/data-protection-engineering" ] ;
    rdfs:isDefinedBy dpv-owl: ;
    rdfs:subClassOf dpv-owl:SecurityMethod ;
    sw:term_status "accepted"@en ;
    skos:definition "Use of synthetic data to preserve privacy, security, or other effects and side-effects"@en ;
    skos:prefLabel "Use of Synthetic Data"@en .

dpv-owl:User a rdfs:Class,
        owl:Class,
        dpv-owl:DataSubject ;
    dct:contributor "Harshvardhan J. Pandit, Georg P. Krog, Julian Flake, Paul Ryan, Beatriz Esteves" ;
    dct:created "2022-04-06"^^xsd:date ;
    rdfs:isDefinedBy dpv-owl: ;
    rdfs:subClassOf dpv-owl:DataSubject ;
    sw:term_status "accepted"@en ;
    skos:definition "Data subjects that use service(s)"@en ;
    skos:prefLabel "User"@en .

dpv-owl:UserInterfacePersonalisation a rdfs:Class,
        owl:Class,
        dpv-owl:Purpose ;
    dct:contributor "Harshvardhan J. Pandit, Javier Fernández, Axel Polleres, Elmar Kiesling, Fajar Ekaputra, Simon Steyskal" ;
    dct:created "2019-04-05"^^xsd:date ;
    rdfs:isDefinedBy dpv-owl: ;
    rdfs:subClassOf dpv-owl:ServicePersonalisation ;
    sw:term_status "accepted"@en ;
    skos:definition "Purposes associated with personalisation of interfaces presented to the user"@en ;
    skos:prefLabel "User Interface Personalisation"@en ;
    skos:scopeNote "Examples of user-interface personalisation include changing the language to match the locale"@en .

dpv-owl:VariableLocation a rdfs:Class,
        owl:Class,
        dpv-owl:LocationFixture ;
    dct:contributor "Harshvardhan J. Pandit" ;
    dct:created "2022-06-15"^^xsd:date ;
    dct:modified "2020-10-05"^^xsd:date ;
    rdfs:isDefinedBy dpv-owl: ;
    rdfs:subClassOf dpv-owl:LocationFixture ;
    sw:term_status "accepted"@en ;
    skos:definition "Location that is known but is variable e.g. somewhere within a given area"@en ;
    skos:prefLabel "Variable Location"@en .

dpv-owl:VendorManagement a rdfs:Class,
        owl:Class,
        dpv-owl:Purpose ;
    dct:contributor "Paul Ryan, Georg P. Krog, David Hickey, Harshvardhan J. Pandit" ;
    dct:created "2021-09-01"^^xsd:date ;
    dct:source [ a schema:WebPage ;
            schema:name "Belgian DPA ROPA Template" ;
            schema:url "https://www.privacycommission.be/nl/model-voor-een-register-van-de-verwerkingsactiviteiten" ] ;
    rdfs:isDefinedBy dpv-owl: ;
    rdfs:subClassOf dpv-owl:Purpose ;
    sw:term_status "accepted"@en ;
    skos:definition "Purposes associated with manage orders, payment, evaluation, and prospecting related to vendors"@en ;
    skos:prefLabel "Vendor Management"@en .

dpv-owl:VendorPayment a rdfs:Class,
        owl:Class,
        dpv-owl:Purpose ;
    dct:contributor "Paul Ryan, Georg P. Krog, David Hickey, Harshvardhan J. Pandit" ;
    dct:created "2021-09-01"^^xsd:date ;
    dct:source [ a schema:WebPage ;
            schema:name "Belgian DPA ROPA Template" ;
            schema:url "https://www.privacycommission.be/nl/model-voor-een-register-van-de-verwerkingsactiviteiten" ] ;
    rdfs:isDefinedBy dpv-owl: ;
    rdfs:subClassOf dpv-owl:VendorManagement ;
    sw:term_status "accepted"@en ;
    skos:definition "Purposes associated with managing payment of vendors"@en ;
    skos:prefLabel "Vendor Payment"@en .

dpv-owl:VendorRecordsManagement a rdfs:Class,
        owl:Class,
        dpv-owl:Purpose ;
    dct:contributor "Paul Ryan, Georg P. Krog, David Hickey, Harshvardhan J. Pandit" ;
    dct:created "2021-09-01"^^xsd:date ;
    dct:source [ a schema:WebPage ;
            schema:name "Belgian DPA ROPA Template" ;
            schema:url "https://www.privacycommission.be/nl/model-voor-een-register-van-de-verwerkingsactiviteiten" ] ;
    rdfs:isDefinedBy dpv-owl: ;
    rdfs:subClassOf dpv-owl:VendorManagement ;
    sw:term_status "accepted"@en ;
    skos:definition "Purposes associated with managing records and orders related to vendors"@en ;
    skos:prefLabel "Vendor Records Management"@en .

dpv-owl:VendorSelectionAssessment a rdfs:Class,
        owl:Class,
        dpv-owl:Purpose ;
    dct:contributor "Paul Ryan, Georg P. Krog, David Hickey, Harshvardhan J. Pandit" ;
    dct:created "2021-09-01"^^xsd:date ;
    dct:source [ a schema:WebPage ;
            schema:name "Belgian DPA ROPA Template" ;
            schema:url "https://www.privacycommission.be/nl/model-voor-een-register-van-de-verwerkingsactiviteiten" ] ;
    rdfs:isDefinedBy dpv-owl: ;
    rdfs:subClassOf dpv-owl:VendorManagement ;
    sw:term_status "accepted"@en ;
    skos:definition "Purposes associated with managing selection, assessment, and evaluation related to vendors"@en ;
    skos:prefLabel "Vendor Selection Assessment"@en .

dpv-owl:Verification a rdfs:Class,
        owl:Class,
        dpv-owl:Purpose ;
    dct:contributor "Beatriz Esteves, Harshvardhan J. Pandit" ;
    dct:created "2024-02-14"^^xsd:date ;
    rdfs:isDefinedBy dpv-owl: ;
    rdfs:subClassOf dpv-owl:EnforceSecurity ;
    sw:term_status "accepted"@en ;
    skos:definition "Purposes association with verification e.g. information, identity, integrity"@en ;
    skos:prefLabel "Verification"@en .

dpv-owl:VerifiedData a rdfs:Class,
        owl:Class ;
    dct:contributor "Harshvardhan J. Pandit" ;
    dct:created "2022-11-02"^^xsd:date ;
    rdfs:isDefinedBy dpv-owl: ;
    rdfs:subClassOf dpv-owl:Data ;
    sw:term_status "accepted"@en ;
    skos:definition "Data that has been verified in terms of accuracy, consistency, or quality"@en ;
    skos:prefLabel "Verified Data"@en .

dpv-owl:VirtualisationSecurity a rdfs:Class,
        owl:Class,
        dpv-owl:TechnicalMeasure ;
    dct:contributor "Harshvardhan J. Pandit" ;
    dct:created "2022-08-17"^^xsd:date ;
    dct:source [ a schema:WebPage ;
            schema:name "ENISA Reference Incident Classification Taxonomy 2018" ;
            schema:url "https://www.enisa.europa.eu/publications/reference-incident-classification-taxonomy/" ] ;
    rdfs:isDefinedBy dpv-owl: ;
    rdfs:subClassOf dpv-owl:SecurityMethod ;
    sw:term_status "accepted"@en ;
    skos:definition "Security implemented at or through virtualised environments"@en ;
    skos:prefLabel "Virtualisation Security"@en .

dpv-owl:Visitor a rdfs:Class,
        owl:Class,
        dpv-owl:DataSubject ;
    dct:contributor "Harshvardhan J. Pandit, Georg P. Krog, Julian Flake, Paul Ryan, Beatriz Esteves" ;
    dct:created "2022-04-06"^^xsd:date ;
    rdfs:isDefinedBy dpv-owl: ;
    rdfs:subClassOf dpv-owl:DataSubject ;
    sw:term_status "accepted"@en ;
    skos:definition "Data subjects that are temporary visitors"@en ;
    skos:prefLabel "Visitor"@en .

dpv-owl:VitalInterest a rdfs:Class,
        owl:Class,
        dpv-owl:LegalBasis ;
    dct:contributor "Harshvardhan J. Pandit" ;
    dct:created "2021-04-21"^^xsd:date ;
    rdfs:isDefinedBy dpv-owl: ;
    rdfs:subClassOf dpv-owl:LegalBasis ;
    sw:term_status "accepted"@en ;
    skos:definition "Activities are necessary or required to protect vital interests of a data subject or other natural person"@en ;
    skos:prefLabel "Vital Interest"@en .

dpv-owl:VitalInterestOfDataSubject a rdfs:Class,
        owl:Class,
        dpv-owl:LegalBasis ;
    dct:contributor "Georg P. Krog, Harshvardhan J. Pandit, Paul Ryan" ;
    dct:created "2021-04-21"^^xsd:date ;
    rdfs:isDefinedBy dpv-owl: ;
    rdfs:subClassOf dpv-owl:VitalInterestOfNaturalPerson ;
    sw:term_status "accepted"@en ;
    skos:definition "Activities are necessary or required to protect vital interests of a data subject"@en ;
    skos:prefLabel "Vital Interest of Data Subject"@en .

dpv-owl:VitalInterestOfNaturalPerson a rdfs:Class,
        owl:Class,
        dpv-owl:LegalBasis ;
    dct:contributor "Georg P. Krog, Harshvardhan J. Pandit, Paul Ryan" ;
    dct:created "2021-04-21"^^xsd:date ;
    rdfs:isDefinedBy dpv-owl: ;
    rdfs:subClassOf dpv-owl:VitalInterest ;
    sw:term_status "accepted"@en ;
    skos:definition "Activities are necessary or required to protect vital interests of a natural person"@en ;
    skos:prefLabel "Vital Interest of Natural Person"@en .

dpv-owl:VulnerabilityTestingMethods a rdfs:Class,
        owl:Class,
        dpv-owl:TechnicalMeasure ;
    dct:contributor "Harshvardhan J. Pandit" ;
    dct:created "2022-08-17"^^xsd:date ;
    dct:source [ a schema:WebPage ;
            schema:name "ENISA Reference Incident Classification Taxonomy 2018" ;
            schema:url "https://www.enisa.europa.eu/publications/reference-incident-classification-taxonomy/" ] ;
    rdfs:isDefinedBy dpv-owl: ;
    rdfs:subClassOf dpv-owl:SecurityMethod ;
    sw:term_status "accepted"@en ;
    skos:definition "Methods that assess or discover vulnerabilities in a system"@en ;
    skos:prefLabel "Vulnerability Testing Methods"@en .

dpv-owl:VulnerableDataSubject a rdfs:Class,
        owl:Class,
        dpv-owl:DataSubject ;
    dct:contributor "Georg P. Krog, Paul Ryan, Harshvardhan J. Pandit" ;
    dct:created "2020-11-04"^^xsd:date ;
    rdfs:isDefinedBy dpv-owl: ;
    rdfs:subClassOf dpv-owl:DataSubject ;
    sw:term_status "accepted"@en ;
    skos:definition "Data Subjects which should be considered 'vulnerable' and therefore would require additional measures and safeguards"@en ;
    skos:prefLabel "Vulnerable Data Subject"@en ;
    skos:scopeNote "This concept denotes a Data Subject or a group are vulnerable, but not what vulnerability they possess or its context. This information can be provided additionally as comments, or as separate concepts and relations. Proposals for this are welcome."@en .

dpv-owl:WebBrowserSecurity a rdfs:Class,
        owl:Class,
        dpv-owl:TechnicalMeasure ;
    dct:contributor "Harshvardhan J. Pandit" ;
    dct:created "2022-08-17"^^xsd:date ;
    dct:source [ a schema:WebPage ;
            schema:name "ENISA Reference Incident Classification Taxonomy 2018" ;
            schema:url "https://www.enisa.europa.eu/publications/reference-incident-classification-taxonomy/" ] ;
    rdfs:isDefinedBy dpv-owl: ;
    rdfs:subClassOf dpv-owl:SecurityMethod ;
    sw:term_status "accepted"@en ;
    skos:definition "Security implemented at or over web browsers"@en ;
    skos:prefLabel "WebBrowser Security"@en .

dpv-owl:WebSecurityProtocols a rdfs:Class,
        owl:Class,
        dpv-owl:TechnicalMeasure ;
    dct:contributor "Harshvardhan J. Pandit" ;
    dct:created "2022-08-17"^^xsd:date ;
    dct:source [ a schema:WebPage ;
            schema:name "ENISA Reference Incident Classification Taxonomy 2018" ;
            schema:url "https://www.enisa.europa.eu/publications/reference-incident-classification-taxonomy/" ] ;
    rdfs:isDefinedBy dpv-owl: ;
    rdfs:subClassOf dpv-owl:SecurityMethod ;
    sw:term_status "accepted"@en ;
    skos:definition "Security implemented at or over web-based protocols"@en ;
    skos:prefLabel "Web Security Protocols"@en .

dpv-owl:WirelessSecurityProtocols a rdfs:Class,
        owl:Class,
        dpv-owl:TechnicalMeasure ;
    dct:contributor "Harshvardhan J. Pandit" ;
    dct:created "2022-08-17"^^xsd:date ;
    dct:source [ a schema:WebPage ;
            schema:name "ENISA Reference Incident Classification Taxonomy 2018" ;
            schema:url "https://www.enisa.europa.eu/publications/reference-incident-classification-taxonomy/" ] ;
    rdfs:isDefinedBy dpv-owl: ;
    rdfs:subClassOf dpv-owl:SecurityMethod ;
    sw:term_status "accepted"@en ;
    skos:definition "Security implemented at or over wireless communication protocols"@en ;
    skos:prefLabel "Wireless Security Protocols"@en .

dpv-owl:WithdrawConsent a rdfs:Class,
        owl:Class ;
    dct:created "2024-05-11"^^xsd:date ;
    rdfs:isDefinedBy dpv-owl: ;
    rdfs:subClassOf dpv-owl:ConsentControl,
        dpv-owl:WithdrawingFromProcess ;
    sw:term_status "accepted"@en ;
    skos:definition "Control for withdrawing consent"@en ;
    skos:prefLabel "Withdraw Consent"@en ;
    skos:scopeNote "Indicates how the data subject can withdraw consent e.g. used with dpv:isExercisedAt"@en .

dpv-owl:WithdrawingFromProcess a rdfs:Class,
        owl:Class,
        dpv-owl:EntityPermissiveInvolvement ;
    dct:contributor "Harshvardhan J. Pandit, Delaram Golpayegani, Steve Hickman" ;
    dct:created "2024-05-11"^^xsd:date ;
    rdfs:isDefinedBy dpv-owl: ;
    rdfs:subClassOf dpv-owl:EntityPermissiveInvolvement ;
    sw:term_status "accepted"@en ;
    skos:definition "Involvement where entity can withdraw a previously given assent from specified context"@en ;
    skos:prefLabel "Withdrawing from Process"@en .

dpv-owl:WithinDevice a rdfs:Class,
        owl:Class,
        dpv-owl:Location ;
    dct:contributor "Harshvardhan J. Pandit" ;
    dct:created "2022-06-15"^^xsd:date ;
    dct:modified "2020-10-05"^^xsd:date ;
    rdfs:isDefinedBy dpv-owl: ;
    rdfs:subClassOf dpv-owl:LocalLocation ;
    sw:term_status "accepted"@en ;
    skos:definition "Location is local and entirely within a device, such as a smartphone"@en ;
    skos:prefLabel "Within Device"@en .

dpv-owl:WithinPhysicalEnvironment a rdfs:Class,
        owl:Class,
        dpv-owl:Location ;
    dct:contributor "Harshvardhan J. Pandit" ;
    dct:created "2020-10-06"^^xsd:date ;
    rdfs:isDefinedBy dpv-owl: ;
    rdfs:subClassOf dpv-owl:LocalLocation ;
    sw:term_status "accepted"@en ;
    skos:definition "Location is local and entirely within a physical environment, such as a room"@en ;
    skos:prefLabel "Within Physical Environment"@en .

dpv-owl:WithinVirtualEnvironment a rdfs:Class,
        owl:Class,
        dpv-owl:Location ;
    dct:contributor "Harshvardhan J. Pandit" ;
    dct:created "2020-10-06"^^xsd:date ;
    rdfs:isDefinedBy dpv-owl: ;
    rdfs:subClassOf dpv-owl:LocalLocation ;
    sw:term_status "accepted"@en ;
    skos:definition "Location is local and entirely within a virtual environment, such as a shared network directory"@en ;
    skos:prefLabel "Within Virtual Environment"@en .

dpv-owl:ZeroKnowledgeAuthentication a rdfs:Class,
        owl:Class,
        dpv-owl:TechnicalMeasure ;
    dct:contributor "Harshvardhan J. Pandit" ;
    dct:created "2022-08-17"^^xsd:date ;
    dct:source [ a schema:WebPage ;
            schema:name "ENISA Data Protection Engineering" ;
            schema:url "https://www.enisa.europa.eu/publications/data-protection-engineering" ] ;
    rdfs:isDefinedBy dpv-owl: ;
    rdfs:subClassOf dpv-owl:AuthenticationProtocols,
        dpv-owl:CryptographicMethods ;
    sw:term_status "accepted"@en ;
    skos:definition "Authentication using Zero-Knowledge proofs"@en ;
    skos:prefLabel "Zero Knowledge Authentication"@en .

dct:accessRights a rdf:Property,
        owl:ObjectProperty ;
    rdfs:isDefinedBy dpv-owl: ;
    skos:prefLabel "dct:accessRights"@en ;
    skos:scopeNote "Also used for specifying constraints on access associated with Rights Exercising (e.g. User must log in) or access to provided data (e.g. access via link)"@en .

dct:format a rdf:Property,
        owl:ObjectProperty ;
    rdfs:isDefinedBy dpv-owl: ;
    skos:prefLabel "dct:format"@en ;
    skos:scopeNote "Also used for specifying the format of provided information, for example a CSV dataset"@en .

dct:hasPart a rdf:Property,
        owl:ObjectProperty ;
    dcam:domainIncludes dpv-owl:RightExerciseRecord ;
    dcam:rangeIncludes dpv-owl:RightExerciseActivity ;
    rdfs:isDefinedBy dpv-owl: ;
    skos:prefLabel "dct:hasPart"@en ;
    skos:scopeNote "Also used for specifying a RightExerciseRecord has RightExerciseActivity as part of its records"@en ;
    schema:domainIncludes dpv-owl:RightExerciseRecord ;
    schema:rangeIncludes dpv-owl:RightExerciseActivity .

dct:isPartOf a rdf:Property,
        owl:ObjectProperty ;
    dcam:domainIncludes dpv-owl:RightExerciseActivity ;
    dcam:rangeIncludes dpv-owl:RightExerciseRecord ;
    rdfs:isDefinedBy dpv-owl: ;
    skos:prefLabel "dct:isPartOf"@en ;
    skos:scopeNote "Also used for specifying a RightExerciseActivity is part of a RightExerciseRecord"@en ;
    schema:domainIncludes dpv-owl:RightExerciseActivity ;
    schema:rangeIncludes dpv-owl:RightExerciseRecord .

dct:valid a rdf:Property,
        owl:ObjectProperty ;
    rdfs:isDefinedBy dpv-owl: ;
    skos:prefLabel "dct:valid"@en ;
    skos:scopeNote "Also used for specifying the temporal validity of an activity associated with Right Exercise. For example, limits on duration for providing or accessing provided information"@en .

foaf:page a rdf:Property,
        owl:ObjectProperty ;
    dcam:domainIncludes dpv-owl:RightExerciseActivity ;
    rdfs:isDefinedBy dpv-owl: ;
    skos:prefLabel "foaf:page"@en ;
    skos:scopeNote "Also used to indicate a web page or document providing information or functionality associated with a Right Exercise"@en ;
    schema:domainIncludes dpv-owl:RightExerciseActivity .

dpv-owl:hasActiveEntity a rdf:Property,
        owl:ObjectProperty ;
    dcam:rangeIncludes dpv-owl:EntityActiveInvolvement ;
    dct:created "2024-05-11"^^xsd:date ;
    rdfs:isDefinedBy dpv-owl: ;
    rdfs:subPropertyOf dpv-owl:hasEntity ;
    sw:term_status "accepted"@en ;
    skos:definition "indicates the entity is actively involved in specified context"@en ;
    skos:prefLabel "has active entity"@en ;
    schema:rangeIncludes dpv-owl:EntityActiveInvolvement .

dpv-owl:hasActivityStatus a rdf:Property,
        owl:ObjectProperty ;
    dcam:rangeIncludes dpv-owl:ActivityStatus ;
    dct:contributor "Harshvardhan J. Pandit" ;
    dct:created "2022-05-18"^^xsd:date ;
    vann:example dex-owl:E0054 ;
    rdfs:isDefinedBy dpv-owl: ;
    rdfs:subPropertyOf dpv-owl:hasStatus ;
    sw:term_status "accepted"@en ;
    skos:definition "Indicates the status of activity of specified concept"@en ;
    skos:prefLabel "has activity status"@en ;
    schema:rangeIncludes dpv-owl:ActivityStatus .

dpv-owl:hasAddress a rdf:Property,
        owl:ObjectProperty ;
    dcam:domainIncludes dpv-owl:Entity ;
    dct:contributor "Harshvardhan J. Pandit, Georg P. Krog, Paul Ryan, Beatriz Esteves" ;
    dct:created "2020-11-04"^^xsd:date ;
    rdfs:isDefinedBy dpv-owl: ;
    sw:term_status "accepted"@en ;
    skos:definition "Specifies address of a legal entity such as street address or pin code"@en ;
    skos:prefLabel "has address"@en ;
    schema:domainIncludes dpv-owl:Entity .

dpv-owl:hasAlgorithmicLogic a rdf:Property,
        owl:ObjectProperty ;
    dcam:rangeIncludes dpv-owl:AlgorithmicLogic ;
    dct:contributor "Georg P. Krog, Paul Ryan, Harshvardhan J. Pandit" ;
    dct:created "2020-11-04"^^xsd:date ;
    dct:modified "2022-06-15"^^xsd:date ;
    rdfs:isDefinedBy dpv-owl: ;
    sw:term_status "accepted"@en ;
    skos:definition "Indicates the logic used in processing such as for automated decision making"@en ;
    skos:prefLabel "has algorithmic logic"@en ;
    schema:rangeIncludes dpv-owl:AlgorithmicLogic .

dpv-owl:hasApplicability a rdf:Property,
        owl:ObjectProperty ;
    dcam:rangeIncludes dpv-owl:Applicability ;
    dct:contributor "Harshvardhan J. Pandit" ;
    dct:created "2023-08-24"^^xsd:date ;
    vann:example dex-owl:E0053 ;
    rdfs:isDefinedBy dpv-owl: ;
    sw:term_status "accepted"@en ;
    skos:definition "Indicates situations where the context is not applicable, information is not available, or this is unknown. An appropriate instance of dpv:Applicability should be used with this relation to express the situation"@en ;
    skos:prefLabel "has applicability"@en ;
    schema:rangeIncludes dpv-owl:Applicability .

dpv-owl:hasApplicableLaw a rdf:Property,
        owl:ObjectProperty ;
    dcam:rangeIncludes dpv-owl:Law ;
    dct:contributor "Harshvardhan J. Pandit" ;
    dct:created "2022-01-19"^^xsd:date ;
    rdfs:isDefinedBy dpv-owl: ;
    sw:term_status "accepted"@en ;
    skos:definition "Indicates applicability of a Law"@en ;
    skos:prefLabel "has applicable law"@en ;
    schema:rangeIncludes dpv-owl:Law .

dpv-owl:hasAuditStatus a rdf:Property,
        owl:ObjectProperty ;
    dcam:rangeIncludes dpv-owl:AuditStatus ;
    dct:contributor "Harshvardhan J. Pandit" ;
    dct:created "2022-06-22"^^xsd:date ;
    vann:example dex-owl:E0056,
        dex-owl:E0057 ;
    rdfs:isDefinedBy dpv-owl: ;
    rdfs:subPropertyOf dpv-owl:hasStatus ;
    sw:term_status "accepted"@en ;
    skos:definition "Indicates the status of audit associated with specified concept"@en ;
    skos:prefLabel "has audit status"@en ;
    schema:rangeIncludes dpv-owl:AuditStatus .

dpv-owl:hasAuthority a rdf:Property,
        owl:ObjectProperty ;
    dcam:rangeIncludes dpv-owl:Authority ;
    dct:contributor "Harshvardhan J. Pandit, Georg P. Krog" ;
    dct:created "2022-01-19"^^xsd:date ;
    rdfs:isDefinedBy dpv-owl: ;
    sw:term_status "accepted"@en ;
    skos:definition "Indicates applicability of authority for a jurisdiction"@en ;
    skos:prefLabel "has authority"@en ;
    schema:rangeIncludes dpv-owl:Authority .

dpv-owl:hasAutomationLevel a rdf:Property,
        owl:ObjectProperty ;
    dcam:rangeIncludes dpv-owl:AutomationLevel ;
    dct:contributor "Harshvardhan J. Pandit" ;
    dct:created "2022-08-13"^^xsd:date ;
    dct:modified "2024-04-20"^^xsd:date ;
    rdfs:isDefinedBy dpv-owl: ;
    sw:term_status "accepted"@en ;
    skos:definition "Indicates the level of automation involved in implementation of the specified context"@en ;
    skos:prefLabel "has automation level"@en ;
    schema:rangeIncludes dpv-owl:AutomationLevel .

dpv-owl:hasConformanceStatus a rdf:Property,
        owl:ObjectProperty ;
    dcam:rangeIncludes dpv-owl:ConformanceStatus ;
    dct:contributor "Harshvardhan J. Pandit" ;
    dct:created "2024-06-10"^^xsd:date ;
    rdfs:isDefinedBy dpv-owl: ;
    sw:term_status "accepted"@en ;
    skos:definition "Indicates the status of being conformant or non-conformant"@en ;
    skos:prefLabel "has conformance status"@en ;
    schema:rangeIncludes dpv-owl:ConformanceStatus .

dpv-owl:hasConsentControl a rdf:Property,
        owl:ObjectProperty ;
    dcam:rangeIncludes dpv-owl:ConsentControl ;
    dct:created "2024-05-11"^^xsd:date ;
    rdfs:isDefinedBy dpv-owl: ;
    sw:term_status "accepted"@en ;
    skos:definition "Specific a control associated with consent"@en ;
    skos:prefLabel "has consent control"@en ;
    schema:rangeIncludes dpv-owl:ConsentControl .

dpv-owl:hasConsentStatus a rdf:Property,
        owl:ObjectProperty ;
    dcam:rangeIncludes dpv-owl:ConsentStatus ;
    dct:contributor "Georg P. Krog, Harshvardhan J. Pandit, Paul Ryan, Julian Flake" ;
    dct:created "2022-06-21"^^xsd:date ;
    rdfs:isDefinedBy dpv-owl: ;
    sw:term_status "accepted"@en ;
    skos:definition "Specifies the state or status of consent"@en ;
    skos:prefLabel "has consent status"@en ;
    schema:rangeIncludes dpv-owl:ConsentStatus .

dpv-owl:hasContact a rdf:Property,
        owl:ObjectProperty ;
    dcam:domainIncludes dpv-owl:Entity ;
    dct:contributor "Harshvardhan J. Pandit, Georg P. Krog, Paul Ryan, Beatriz Esteves" ;
    dct:created "2020-11-04"^^xsd:date ;
    rdfs:isDefinedBy dpv-owl: ;
    sw:term_status "accepted"@en ;
    skos:definition "Specifies contact details of a legal entity such as phone  or email"@en ;
    skos:prefLabel "has contact"@en ;
    schema:domainIncludes dpv-owl:Entity .

dpv-owl:hasContext a rdf:Property,
        owl:ObjectProperty ;
    dcam:rangeIncludes dpv-owl:Context ;
    dct:created "2019-04-05"^^xsd:date ;
    rdfs:isDefinedBy dpv-owl: ;
    sw:term_status "accepted"@en ;
    skos:definition "Indicates a purpose is restricted to the specified context(s)"@en ;
    skos:prefLabel "has context"@en ;
    schema:rangeIncludes dpv-owl:Context .

dpv-owl:hasDataExporter a rdf:Property,
        owl:ObjectProperty ;
    dcam:rangeIncludes dpv-owl:DataExporter ;
    dct:contributor "Paul Ryan, Georg P. Krog, Harshvardhan J. Pandit" ;
    dct:created "2022-02-09"^^xsd:date ;
    rdfs:isDefinedBy dpv-owl: ;
    rdfs:subPropertyOf dpv-owl:hasEntity ;
    sw:term_status "accepted"@en ;
    skos:definition "Indicates inclusion or applicability of a LegalEntity in the role of Data Exporter"@en ;
    skos:prefLabel "has data exporter"@en ;
    schema:rangeIncludes dpv-owl:DataExporter .

dpv-owl:hasDataImporter a rdf:Property,
        owl:ObjectProperty ;
    dcam:rangeIncludes dpv-owl:DataImporter ;
    dct:contributor "Paul Ryan, Georg P. Krog, Harshvardhan J. Pandit" ;
    dct:created "2022-02-09"^^xsd:date ;
    rdfs:isDefinedBy dpv-owl: ;
    rdfs:subPropertyOf dpv-owl:hasRecipient ;
    sw:term_status "accepted"@en ;
    skos:definition "Indicates inclusion or applicability of a LegalEntity in the role of Data Importer"@en ;
    skos:prefLabel "has data importer"@en ;
    schema:rangeIncludes dpv-owl:DataImporter .

dpv-owl:hasDataProcessor a rdf:Property,
        owl:ObjectProperty ;
    dcam:rangeIncludes dpv-owl:DataProcessor ;
    dct:contributor "Paul Ryan, Georg P. Krog, Harshvardhan J. Pandit" ;
    dct:created "2022-02-09"^^xsd:date ;
    rdfs:isDefinedBy dpv-owl: ;
    rdfs:subPropertyOf dpv-owl:hasRecipient ;
    sw:term_status "accepted"@en ;
    skos:definition "Indiciates inclusion or applicability of a Data Processor"@en ;
    skos:prefLabel "has data processor"@en ;
    schema:rangeIncludes dpv-owl:DataProcessor .

dpv-owl:hasDataProtectionOfficer a rdf:Property,
        owl:ObjectProperty ;
    dcam:rangeIncludes dpv-owl:DataProtectionOfficer ;
    dct:contributor "Paul Ryan, Rob Brennan" ;
    dct:created "2022-03-02"^^xsd:date ;
    rdfs:isDefinedBy dpv-owl: ;
    rdfs:subPropertyOf dpv-owl:hasRepresentative ;
    sw:term_status "accepted"@en ;
    skos:definition "Specifies an associated data protection officer"@en ;
    skos:prefLabel "has data protection officer"@en ;
    schema:rangeIncludes dpv-owl:DataProtectionOfficer .

dpv-owl:hasDataSource a rdf:Property,
        owl:ObjectProperty ;
    dcam:rangeIncludes dpv-owl:DataSource ;
    dct:contributor "Georg P. Krog, Paul Ryan, Harshvardhan J. Pandit" ;
    dct:created "2020-11-04"^^xsd:date ;
    rdfs:isDefinedBy dpv-owl: ;
    sw:term_status "accepted"@en ;
    skos:definition "Indicates the source or origin of data being processed"@en ;
    skos:prefLabel "has data source"@en ;
    schema:rangeIncludes dpv-owl:DataSource .

dpv-owl:hasDataSubject a rdf:Property,
        owl:ObjectProperty ;
    dcam:rangeIncludes dpv-owl:DataSubject ;
    dct:contributor "Axel Polleres, Javier Fernández, Harshvardhan J. Pandit, Mark Lizar, Bud Bruegger" ;
    dct:created "2019-04-04"^^xsd:date ;
    dct:modified "2020-11-04"^^xsd:date ;
    rdfs:isDefinedBy dpv-owl: ;
    rdfs:subPropertyOf dpv-owl:hasEntity ;
    sw:term_status "accepted"@en ;
    skos:definition "Indicates association with Data Subject"@en ;
    skos:prefLabel "has data subject"@en ;
    schema:rangeIncludes dpv-owl:DataSubject .

dpv-owl:hasDataSubjectScale a rdf:Property,
        owl:ObjectProperty ;
    dcam:rangeIncludes dpv-owl:DataSubjectScale ;
    dct:contributor "Harshvardhan J. Pandit" ;
    dct:created "2022-06-22"^^xsd:date ;
    rdfs:isDefinedBy dpv-owl: ;
    rdfs:subPropertyOf dpv-owl:hasScale ;
    sw:term_status "accepted"@en ;
    skos:definition "Indicates the scale of data subjects"@en ;
    skos:prefLabel "has data subject scale"@en ;
    schema:rangeIncludes dpv-owl:DataSubjectScale .

dpv-owl:hasDataVolume a rdf:Property,
        owl:ObjectProperty ;
    dcam:rangeIncludes dpv-owl:DataVolume ;
    dct:contributor "Harshvardhan J. Pandit" ;
    dct:created "2022-06-22"^^xsd:date ;
    rdfs:isDefinedBy dpv-owl: ;
    rdfs:subPropertyOf dpv-owl:hasScale ;
    sw:term_status "accepted"@en ;
    skos:definition "Indicates the volume of data"@en ;
    skos:prefLabel "has data volume"@en ;
    schema:rangeIncludes dpv-owl:DataVolume .

dpv-owl:hasDuration a rdf:Property,
        owl:ObjectProperty ;
    dcam:rangeIncludes dpv-owl:Duration ;
    dct:contributor "Axel Polleres, Rob Brennan, Harshvardhan J. Pandit, Mark Lizar" ;
    dct:created "2019-04-05"^^xsd:date ;
    dct:source [ a schema:WebPage ;
            schema:name "SPECIAL Project" ;
            schema:url "https://specialprivacy.ercim.eu/" ] ;
    vann:example dex-owl:E0050,
        dex-owl:E0070 ;
    rdfs:isDefinedBy dpv-owl: ;
    sw:term_status "accepted"@en ;
    skos:definition "Indicates information about duration"@en ;
    skos:prefLabel "has duration"@en ;
    schema:rangeIncludes dpv-owl:Duration .

dpv-owl:hasEntityControl a rdf:Property,
        owl:ObjectProperty ;
    dcam:rangeIncludes dpv-owl:EntityControl ;
    dct:contributor "Harshvardhan J. Pandit" ;
    dct:created "2024-04-14"^^xsd:date ;
    rdfs:isDefinedBy dpv-owl: ;
    rdfs:subPropertyOf dpv-owl:hasTechnicalOrganisationalMeasure ;
    sw:term_status "accepted"@en ;
    skos:definition "Indicates a control or measure provided for an entity to perform the specified action"@en ;
    skos:prefLabel "has entity control"@en ;
    schema:rangeIncludes dpv-owl:EntityControl .

dpv-owl:hasEntityInvolvement a rdf:Property,
        owl:ObjectProperty ;
    dcam:rangeIncludes dpv-owl:EntityInvolvement ;
    dct:created "2024-05-11"^^xsd:date ;
    rdfs:isDefinedBy dpv-owl: ;
    sw:term_status "accepted"@en ;
    skos:definition "Indicates involvement of an entity in specified context"@en ;
    skos:prefLabel "has entity involvement"@en ;
    schema:rangeIncludes dpv-owl:EntityInvolvement .

dpv-owl:hasExpectation a rdf:Property,
        owl:ObjectProperty ;
    dcam:rangeIncludes dpv-owl:ExpectationStatus ;
    dct:contributor "Harshvardhan J. Pandit" ;
    dct:created "2024-05-10"^^xsd:date ;
    dct:modified "2024-06-10"^^xsd:date ;
    rdfs:isDefinedBy dpv-owl: ;
    rdfs:subPropertyOf dpv-owl:hasStatus ;
    sw:term_status "accepted"@en ;
    skos:definition "Indicates whether the specified context was expected or unexpected"@en ;
    skos:prefLabel "has expectation"@en ;
    schema:rangeIncludes dpv-owl:ExpectationStatus .

dpv-owl:hasFrequency a rdf:Property,
        owl:ObjectProperty ;
    dcam:rangeIncludes dpv-owl:Frequency ;
    dct:contributor "Harshvardhan J. Pandit" ;
    dct:created "2022-02-16"^^xsd:date ;
    vann:example dex-owl:E0051 ;
    rdfs:isDefinedBy dpv-owl: ;
    sw:term_status "accepted"@en ;
    skos:definition "Indicates the frequency with which something takes place"@en ;
    skos:prefLabel "has frequency"@en ;
    schema:rangeIncludes dpv-owl:Frequency .

dpv-owl:hasGeographicCoverage a rdf:Property,
        owl:ObjectProperty ;
    dcam:rangeIncludes dpv-owl:GeographicCoverage ;
    dct:contributor "Harshvardhan J. Pandit" ;
    dct:created "2022-06-22"^^xsd:date ;
    rdfs:isDefinedBy dpv-owl: ;
    rdfs:subPropertyOf dpv-owl:hasScale ;
    sw:term_status "accepted"@en ;
    skos:definition "Indicate the geographic coverage (of specified context)"@en ;
    skos:prefLabel "has geographic coverage"@en ;
    schema:rangeIncludes dpv-owl:GeographicCoverage .

dpv-owl:hasHumanInvolvement a rdf:Property,
        owl:ObjectProperty ;
    dcam:rangeIncludes dpv-owl:HumanInvolvement ;
    dct:contributor "Georg P. Krog, Paul Ryan, Harshvardhan J. Pandit" ;
    dct:created "2020-11-04"^^xsd:date ;
    rdfs:isDefinedBy dpv-owl: ;
    sw:term_status "accepted"@en ;
    skos:definition "Indicates Involvement of humans in processing such as within automated decision making process"@en ;
    skos:prefLabel "has human involvement"@en ;
    skos:scopeNote "Human involvement is also relevant to 'human in the loop'"@en ;
    schema:rangeIncludes dpv-owl:HumanInvolvement .

dpv-owl:hasIdentifier a rdf:Property,
        owl:ObjectProperty ;
    dct:contributor "Harshvardhan J. Pandit, Georg P. Krog, Paul Ryan, Beatriz Esteves" ;
    dct:created "2020-11-25"^^xsd:date ;
    rdfs:isDefinedBy dpv-owl: ;
    sw:term_status "accepted"@en ;
    skos:definition "Indicates an identifier associated for identification or reference"@en ;
    skos:prefLabel "has identifier"@en .

dpv-owl:hasImpact a rdf:Property,
        owl:ObjectProperty ;
    dcam:rangeIncludes dpv-owl:Impact ;
    dct:contributor "Harshvardhan J. Pandit, Julian Flake, Georg P. Krog, Fajar Ekaputra, Beatriz Esteves" ;
    dct:created "2022-05-18"^^xsd:date ;
    vann:example dex-owl:E0068,
        dex-owl:E0069 ;
    rdfs:isDefinedBy dpv-owl: ;
    rdfs:subPropertyOf dpv-owl:hasConsequence ;
    sw:term_status "accepted"@en ;
    skos:definition "Indicates impact(s) possible or arising as consequences from specified concept"@en ;
    skos:prefLabel "has impact"@en ;
    schema:rangeIncludes dpv-owl:Impact .

dpv-owl:hasImpactAssessment a rdf:Property,
        owl:ObjectProperty ;
    dcam:rangeIncludes dpv-owl:ImpactAssessment ;
    dct:contributor "Harshvardhan J. Pandit" ;
    dct:created "2024-04-14"^^xsd:date ;
    rdfs:isDefinedBy dpv-owl: ;
    rdfs:subPropertyOf dpv-owl:hasAssessment ;
    sw:term_status "accepted"@en ;
    skos:definition "Indicates an impact assessment associated with the specific context"@en ;
    skos:prefLabel "has impact assessment"@en ;
    schema:rangeIncludes dpv-owl:ImpactAssessment .

dpv-owl:hasImpactOn a rdf:Property,
        owl:ObjectProperty ;
    dcam:domainIncludes dpv-owl:Impact ;
    dct:contributor "Harshvardhan J. Pandit, Julian Flake, Georg P. Krog, Fajar Ekaputra, Beatriz Esteves" ;
    dct:created "2022-05-18"^^xsd:date ;
    vann:example dex-owl:E0068 ;
    rdfs:isDefinedBy dpv-owl: ;
    rdfs:subPropertyOf dpv-owl:hasConsequenceOn ;
    sw:term_status "accepted"@en ;
    skos:definition "Indicates the thing (e.g. plan, process, or entity) affected by an impact"@en ;
    skos:prefLabel "has impact on"@en ;
    schema:domainIncludes dpv-owl:Impact .

dpv-owl:hasImportance a rdf:Property,
        owl:ObjectProperty ;
    dcam:rangeIncludes dpv-owl:Importance ;
    dct:contributor "Harshvardhan J. Pandit" ;
    dct:created "2024-04-13"^^xsd:date ;
    rdfs:isDefinedBy dpv-owl: ;
    sw:term_status "accepted"@en ;
    skos:definition "Indicates the importance for specified context or criteria"@en ;
    skos:prefLabel "has importance"@en ;
    schema:rangeIncludes dpv-owl:Importance .

dpv-owl:hasIndicationMethod a rdf:Property,
        owl:ObjectProperty ;
    dct:contributor "Georg P. Krog, Harshvardhan J. Pandit, Paul Ryan, Julian Flake" ;
    dct:created "2022-06-21"^^xsd:date ;
    rdfs:isDefinedBy dpv-owl: ;
    sw:term_status "accepted"@en ;
    skos:definition "Specifies the method by which an entity has indicated the specific context"@en ;
    skos:prefLabel "has indication method"@en .

dpv-owl:hasInformedStatus a rdf:Property,
        owl:ObjectProperty ;
    dcam:rangeIncludes dpv-owl:EntityInformedStatus ;
    dct:contributor "Harshvardhan J. Pandit" ;
    dct:created "2024-05-10"^^xsd:date ;
    rdfs:isDefinedBy dpv-owl: ;
    rdfs:subPropertyOf dpv-owl:hasStatus ;
    sw:term_status "accepted"@en ;
    skos:definition "Indicates whether an entity was informed or uninformed"@en ;
    skos:prefLabel "has informed status"@en ;
    schema:rangeIncludes dpv-owl:EntityInformedStatus .

dpv-owl:hasIntention a rdf:Property,
        owl:ObjectProperty ;
    dcam:rangeIncludes dpv-owl:IntentionStatus ;
    dct:contributor "Harshvardhan J. Pandit" ;
    dct:created "2024-05-10"^^xsd:date ;
    rdfs:isDefinedBy dpv-owl: ;
    rdfs:subPropertyOf dpv-owl:hasStatus ;
    sw:term_status "accepted"@en ;
    skos:definition "Indicates whether the specified context was intended or unintended"@en ;
    skos:prefLabel "has intention"@en ;
    schema:rangeIncludes dpv-owl:IntentionStatus .

dpv-owl:hasInvolvement a rdf:Property,
        owl:ObjectProperty ;
    dcam:rangeIncludes dpv-owl:InvolvementStatus ;
    dct:contributor "Harshvardhan J. Pandit" ;
    dct:created "2024-05-10"^^xsd:date ;
    rdfs:isDefinedBy dpv-owl: ;
    rdfs:subPropertyOf dpv-owl:hasStatus ;
    sw:term_status "accepted"@en ;
    skos:definition "Indicates the involvement status for the specified context"@en ;
    skos:prefLabel "has involvement"@en ;
    schema:rangeIncludes dpv-owl:InvolvementStatus .

dpv-owl:hasJointDataControllers a rdf:Property,
        owl:ObjectProperty ;
    dcam:rangeIncludes dpv-owl:JointDataControllers ;
    dct:contributor "Paul Ryan, Georg P. Krog, Harshvardhan J. Pandit" ;
    dct:created "2022-02-09"^^xsd:date ;
    rdfs:isDefinedBy dpv-owl: ;
    rdfs:subPropertyOf dpv-owl:hasDataController ;
    sw:term_status "accepted"@en ;
    skos:definition "Indicates inclusion or applicability of a Joint Data Controller"@en ;
    skos:prefLabel "has joint data controllers"@en ;
    schema:rangeIncludes dpv-owl:JointDataControllers .

dpv-owl:hasJurisdiction a rdf:Property,
        owl:ObjectProperty ;
    dcam:rangeIncludes dpv-owl:Location ;
    dct:contributor "Harshvardhan J. Pandit" ;
    dct:created "2022-01-19"^^xsd:date ;
    rdfs:isDefinedBy dpv-owl: ;
    sw:term_status "accepted"@en ;
    skos:definition "Indicates applicability of specified jurisdiction"@en ;
    skos:prefLabel "has jurisdiction"@en ;
    schema:rangeIncludes dpv-owl:Location .

dpv-owl:hasJustification a rdf:Property,
        owl:ObjectProperty ;
    dcam:domainIncludes dpv-owl:RightExerciseActivity ;
    dcam:rangeIncludes dpv-owl:Justification ;
    dct:contributor "Harshvardhan J. Pandit" ;
    dct:created "2022-06-15"^^xsd:date ;
    vann:example dex-owl:E0057,
        dex-owl:E0058,
        dex-owl:E0059,
        dex-owl:E0061,
        dex-owl:E0062,
        dex-owl:E0063 ;
    rdfs:isDefinedBy dpv-owl: ;
    sw:term_status "accepted"@en ;
    skos:definition "Indicates a justification for specified concept or context"@en ;
    skos:prefLabel "has justification"@en ;
    skos:scopeNote "Also used for specifying a justification for non-fulfilment of Right Exercise"@en ;
    schema:domainIncludes dpv-owl:RightExerciseActivity ;
    schema:rangeIncludes dpv-owl:Justification .

dpv-owl:hasLawfulness a rdf:Property,
        owl:ObjectProperty ;
    dcam:rangeIncludes dpv-owl:Lawfulness ;
    dct:contributor "Harshvardhan J. Pandit" ;
    dct:created "2022-10-22"^^xsd:date ;
    rdfs:isDefinedBy dpv-owl: ;
    rdfs:subPropertyOf dpv-owl:hasComplianceStatus ;
    sw:term_status "accepted"@en ;
    skos:definition "Indicates the status of being lawful or legally compliant"@en ;
    skos:prefLabel "has lawfulness"@en ;
    schema:rangeIncludes dpv-owl:Lawfulness .

dpv-owl:hasLegalBasis a rdf:Property,
        owl:ObjectProperty ;
    dcam:rangeIncludes dpv-owl:LegalBasis ;
    dct:contributor "Axel Polleres, Javier Fernández" ;
    dct:created "2019-04-04"^^xsd:date ;
    dct:modified "2020-11-04"^^xsd:date ;
    rdfs:isDefinedBy dpv-owl: ;
    sw:term_status "accepted"@en ;
    skos:definition "Indicates use or applicability of a Legal Basis"@en ;
    skos:prefLabel "has legal basis"@en ;
    schema:rangeIncludes dpv-owl:LegalBasis .

dpv-owl:hasLegalMeasure a rdf:Property,
        owl:ObjectProperty ;
    dcam:rangeIncludes dpv-owl:LegalMeasure ;
    dct:created "2023-12-10"^^xsd:date ;
    rdfs:isDefinedBy dpv-owl: ;
    rdfs:subPropertyOf dpv-owl:hasOrganisationalMeasure ;
    sw:term_status "accepted"@en ;
    skos:definition "Indicates use or applicability of Legal measure"@en ;
    skos:prefLabel "has legal measure"@en ;
    schema:rangeIncludes dpv-owl:LegalMeasure .

dpv-owl:hasLikelihood a rdf:Property,
        owl:ObjectProperty ;
    dcam:rangeIncludes dpv-owl:Likelihood ;
    dct:contributor "Harshvardhan J. Pandit, Georg P. Krog, Paul Ryan, Julian Flake" ;
    dct:created "2022-07-20"^^xsd:date ;
    vann:example dex-owl:E0068 ;
    rdfs:isDefinedBy dpv-owl: ;
    sw:term_status "accepted"@en ;
    skos:definition "Indicates the likelihood associated with a concept"@en ;
    skos:prefLabel "has likelihood"@en ;
    schema:rangeIncludes dpv-owl:Likelihood .

dpv-owl:hasName a rdf:Property,
        owl:ObjectProperty ;
    dcam:domainIncludes dpv-owl:Entity ;
    dct:contributor "Harshvardhan J. Pandit, Georg P. Krog, Paul Ryan, Beatriz Esteves" ;
    dct:created "2020-11-04"^^xsd:date ;
    rdfs:isDefinedBy dpv-owl: ;
    sw:term_status "accepted"@en ;
    skos:definition "Specifies name of a legal entity"@en ;
    skos:prefLabel "has name"@en ;
    schema:domainIncludes dpv-owl:Entity .

dpv-owl:hasNecessity a rdf:Property,
        owl:ObjectProperty ;
    dcam:rangeIncludes dpv-owl:Necessity ;
    dct:contributor "Harshvardhan J. Pandit" ;
    dct:created "2024-04-13"^^xsd:date ;
    vann:example dex-owl:E0052 ;
    rdfs:isDefinedBy dpv-owl: ;
    sw:term_status "accepted"@en ;
    skos:definition "Indicates the necessity for specified context or criteria"@en ;
    skos:prefLabel "has necessity"@en ;
    schema:rangeIncludes dpv-owl:Necessity .

dpv-owl:hasNonInvolvedEntity a rdf:Property,
        owl:ObjectProperty ;
    dcam:rangeIncludes dpv-owl:EntityNoInvolvement ;
    dct:created "2024-05-11"^^xsd:date ;
    rdfs:isDefinedBy dpv-owl: ;
    rdfs:subPropertyOf dpv-owl:hasEntity ;
    sw:term_status "accepted"@en ;
    skos:definition "indicates the entity is not involved in specified context"@en ;
    skos:prefLabel "has non-involved entity"@en ;
    schema:rangeIncludes dpv-owl:EntityNoInvolvement .

dpv-owl:hasNonPersonalDataProcess a rdf:Property,
        owl:ObjectProperty ;
    dcam:rangeIncludes dpv-owl:NonPersonalDataProcess ;
    dct:contributor "Harshvardhan J. Pandit" ;
    dct:created "2023-12-12"^^xsd:date ;
    rdfs:isDefinedBy dpv-owl: ;
    sw:term_status "accepted"@en ;
    skos:definition "Indicates association with a Non-Personal Data Process"@en ;
    skos:prefLabel "has non-personal data process"@en ;
    schema:rangeIncludes dpv-owl:NonPersonalDataProcess .

dpv-owl:hasNotice a rdf:Property,
        owl:ObjectProperty ;
    dcam:rangeIncludes dpv-owl:Notice ;
    dct:contributor "Georg P. Krog, Harshvardhan J. Pandit, Paul Ryan, Julian Flake" ;
    dct:created "2022-06-22"^^xsd:date ;
    rdfs:isDefinedBy dpv-owl: ;
    rdfs:subPropertyOf dpv-owl:hasOrganisationalMeasure ;
    sw:term_status "accepted"@en ;
    skos:definition "Indicates the use or applicability of a Notice for the specified context"@en ;
    skos:prefLabel "has notice"@en ;
    schema:rangeIncludes dpv-owl:Notice .

dpv-owl:hasNotificationStatus a rdf:Property,
        owl:ObjectProperty ;
    dcam:rangeIncludes dpv-owl:NotificationStatus ;
    dct:contributor "Harshvardhan J. Pandit" ;
    dct:created "2024-06-10"^^xsd:date ;
    rdfs:isDefinedBy dpv-owl: ;
    sw:term_status "accepted"@en ;
    skos:definition "Indicates the status associated with a notice"@en ;
    skos:prefLabel "has notification status"@en ;
    schema:rangeIncludes dpv-owl:NotificationStatus .

dpv-owl:hasObligation a rdf:Property,
        owl:ObjectProperty ;
    dcam:domainIncludes dpv-owl:Context ;
    dcam:rangeIncludes dpv-owl:Obligation ;
    dct:contributor "Harshvardhan J. Pandit, Georg P. Krog, Beatriz Esteves, Paul Ryan" ;
    dct:created "2022-10-19"^^xsd:date ;
    rdfs:isDefinedBy dpv-owl: ;
    rdfs:subPropertyOf dpv-owl:hasRule ;
    sw:term_status "accepted"@en ;
    skos:definition "Specifying applicability or inclusion of an obligation rule within specified context"@en ;
    skos:prefLabel "has obligation"@en ;
    schema:domainIncludes dpv-owl:Context ;
    schema:rangeIncludes dpv-owl:Obligation .

dpv-owl:hasOrganisationalUnit a rdf:Property,
        owl:ObjectProperty ;
    dcam:domainIncludes dpv-owl:Entity ;
    dcam:rangeIncludes dpv-owl:OrganisationalUnit ;
    dct:contributor "Harshvardhan J. Pandit" ;
    dct:created "2024-06-10"^^xsd:date ;
    rdfs:isDefinedBy dpv-owl: ;
    rdfs:subPropertyOf dpv-owl:hasEntity ;
    sw:term_status "accepted"@en ;
    skos:definition "Indicates the specified entity is a unit of the organisation"@en ;
    skos:prefLabel "has organisational unit"@en ;
    schema:domainIncludes dpv-owl:Entity ;
    schema:rangeIncludes dpv-owl:OrganisationalUnit .

dpv-owl:hasOutcome a rdf:Property,
        owl:ObjectProperty ;
    dct:contributor "Harshvardhan J. Pandit" ;
    dct:created "2022-05-18"^^xsd:date ;
    rdfs:isDefinedBy dpv-owl: ;
    sw:term_status "accepted"@en ;
    skos:definition "Indicates an outcome of specified concept or context"@en ;
    skos:prefLabel "has outcome"@en .

dpv-owl:hasPassiveEntity a rdf:Property,
        owl:ObjectProperty ;
    dcam:rangeIncludes dpv-owl:EntityPassiveInvolvement ;
    dct:created "2024-05-11"^^xsd:date ;
    rdfs:isDefinedBy dpv-owl: ;
    rdfs:subPropertyOf dpv-owl:hasEntity ;
    sw:term_status "accepted"@en ;
    skos:definition "indicates the entity is passively involved in specified context"@en ;
    skos:prefLabel "has passive entity"@en ;
    schema:rangeIncludes dpv-owl:EntityPassiveInvolvement .

dpv-owl:hasPermission a rdf:Property,
        owl:ObjectProperty ;
    dcam:domainIncludes dpv-owl:Context ;
    dcam:rangeIncludes dpv-owl:Permission ;
    dct:contributor "Harshvardhan J. Pandit, Georg P. Krog, Beatriz Esteves, Paul Ryan" ;
    dct:created "2022-10-19"^^xsd:date ;
    vann:example dex-owl:E0066 ;
    rdfs:isDefinedBy dpv-owl: ;
    rdfs:subPropertyOf dpv-owl:hasRule ;
    sw:term_status "accepted"@en ;
    skos:definition "Specifying applicability or inclusion of a permission rule within specified context"@en ;
    skos:prefLabel "has permission"@en ;
    schema:domainIncludes dpv-owl:Context ;
    schema:rangeIncludes dpv-owl:Permission .

dpv-owl:hasPersonalData a rdf:Property,
        owl:ObjectProperty ;
    dcam:rangeIncludes dpv-owl:PersonalData ;
    dct:contributor "Harshvardhan J. Pandit" ;
    dct:created "2022-01-19"^^xsd:date ;
    vann:example dex-owl:E0044 ;
    rdfs:isDefinedBy dpv-owl: ;
    rdfs:subPropertyOf dpv-owl:hasData ;
    sw:term_status "accepted"@en ;
    skos:definition "Indicates association with Personal Data"@en ;
    skos:prefLabel "has personal data"@en ;
    schema:rangeIncludes dpv-owl:PersonalData .

dpv-owl:hasPersonalDataHandling a rdf:Property,
        owl:ObjectProperty ;
    dcam:rangeIncludes dpv-owl:PersonalDataHandling ;
    dct:contributor "Harshvardhan J. Pandit, Georg P. Krog" ;
    dct:created "2022-01-19"^^xsd:date ;
    rdfs:isDefinedBy dpv-owl: ;
    sw:term_status "accepted"@en ;
    skos:definition "Indicates association with Personal Data Handling"@en ;
    skos:prefLabel "has personal data handling"@en ;
    schema:rangeIncludes dpv-owl:PersonalDataHandling .

dpv-owl:hasPersonalDataProcess a rdf:Property,
        owl:ObjectProperty ;
    dcam:rangeIncludes dpv-owl:PersonalDataProcess ;
    dct:contributor "Harshvardhan J. Pandit" ;
    dct:created "2023-12-11"^^xsd:date ;
    rdfs:isDefinedBy dpv-owl: ;
    sw:term_status "accepted"@en ;
    skos:definition "Indicates association with a Personal Data Process"@en ;
    skos:prefLabel "has personal data process"@en ;
    schema:rangeIncludes dpv-owl:PersonalDataProcess .

dpv-owl:hasPhysicalMeasure a rdf:Property,
        owl:ObjectProperty ;
    dcam:rangeIncludes dpv-owl:PhysicalMeasure ;
    dct:created "2023-12-10"^^xsd:date ;
    rdfs:isDefinedBy dpv-owl: ;
    rdfs:subPropertyOf dpv-owl:hasTechnicalOrganisationalMeasure ;
    sw:term_status "accepted"@en ;
    skos:definition "Indicates use or applicability of Physical measure"@en ;
    skos:prefLabel "has physical measure"@en ;
    schema:rangeIncludes dpv-owl:PhysicalMeasure .

dpv-owl:hasPolicy a rdf:Property,
        owl:ObjectProperty ;
    dcam:rangeIncludes dpv-owl:Policy ;
    dct:contributor "Harshvardhan J. Pandit" ;
    dct:created "2022-01-26"^^xsd:date ;
    rdfs:isDefinedBy dpv-owl: ;
    rdfs:subPropertyOf dpv-owl:hasTechnicalOrganisationalMeasure ;
    sw:term_status "accepted"@en ;
    skos:definition "Indicates policy applicable or used"@en ;
    skos:prefLabel "has policy"@en ;
    schema:rangeIncludes dpv-owl:Policy .

dpv-owl:hasProcess a rdf:Property,
        owl:ObjectProperty ;
    dcam:rangeIncludes dpv-owl:Process ;
    dct:contributor "Harshvardhan J. Pandit" ;
    dct:created "2023-12-10"^^xsd:date ;
    rdfs:isDefinedBy dpv-owl: ;
    sw:term_status "accepted"@en ;
    skos:definition "Indicates association with a Process"@en ;
    skos:prefLabel "has process"@en ;
    schema:rangeIncludes dpv-owl:Process .

dpv-owl:hasProcessing a rdf:Property,
        owl:ObjectProperty ;
    dcam:rangeIncludes dpv-owl:Processing ;
    dct:contributor "Axel Polleres, Javier Fernández, Harshvardhan J. Pandit, Mark Lizar, Bud Bruegger" ;
    dct:created "2019-04-04"^^xsd:date ;
    dct:modified "2020-11-04"^^xsd:date ;
    dct:source [ a schema:WebPage ;
            schema:name "SPECIAL Project" ;
            schema:url "https://specialprivacy.ercim.eu/" ] ;
    rdfs:isDefinedBy dpv-owl: ;
    sw:term_status "accepted"@en ;
    skos:definition "Indicates association with Processing"@en ;
    skos:prefLabel "has processing"@en ;
    schema:rangeIncludes dpv-owl:Processing .

dpv-owl:hasProhibition a rdf:Property,
        owl:ObjectProperty ;
    dcam:domainIncludes dpv-owl:Context ;
    dcam:rangeIncludes dpv-owl:Prohibition ;
    dct:contributor "Harshvardhan J. Pandit, Georg P. Krog, Beatriz Esteves, Paul Ryan" ;
    dct:created "2022-10-19"^^xsd:date ;
    vann:example dex-owl:E0066 ;
    rdfs:isDefinedBy dpv-owl: ;
    rdfs:subPropertyOf dpv-owl:hasRule ;
    sw:term_status "accepted"@en ;
    skos:definition "Specifying applicability or inclusion of a prohibition rule within specified context"@en ;
    skos:prefLabel "has prohibition"@en ;
    schema:domainIncludes dpv-owl:Context ;
    schema:rangeIncludes dpv-owl:Prohibition .

dpv-owl:hasPurpose a rdf:Property,
        owl:ObjectProperty ;
    dcam:rangeIncludes dpv-owl:Purpose ;
    dct:contributor "Axel Polleres, Javier Fernández, Harshvardhan J. Pandit, Mark Lizar, Bud Bruegger" ;
    dct:created "2019-04-04"^^xsd:date ;
    dct:modified "2020-11-04"^^xsd:date ;
    dct:source [ a schema:WebPage ;
            schema:name "SPECIAL Project" ;
            schema:url "https://specialprivacy.ercim.eu/" ] ;
    rdfs:isDefinedBy dpv-owl: ;
    sw:term_status "accepted"@en ;
    skos:definition "Indicates association with Purpose"@en ;
    skos:prefLabel "has purpose"@en ;
    schema:rangeIncludes dpv-owl:Purpose .

dpv-owl:hasRecipientDataController a rdf:Property,
        owl:ObjectProperty ;
    dcam:rangeIncludes dpv-owl:DataController ;
    dct:contributor "Paul Ryan, Georg P. Krog, Harshvardhan J. Pandit" ;
    dct:created "2022-02-09"^^xsd:date ;
    rdfs:isDefinedBy dpv-owl: ;
    rdfs:subPropertyOf dpv-owl:hasRecipient ;
    sw:term_status "accepted"@en ;
    skos:definition "Indiciates inclusion or applicability of a Data Controller as a Recipient of persona data"@en ;
    skos:prefLabel "has recipient data controller"@en ;
    schema:rangeIncludes dpv-owl:DataController .

dpv-owl:hasRecipientThirdParty a rdf:Property,
        owl:ObjectProperty ;
    dcam:rangeIncludes dpv-owl:ThirdParty ;
    dct:contributor "Paul Ryan, Georg P. Krog, Harshvardhan J. Pandit" ;
    dct:created "2022-02-09"^^xsd:date ;
    rdfs:isDefinedBy dpv-owl: ;
    rdfs:subPropertyOf dpv-owl:hasRecipient ;
    sw:term_status "accepted"@en ;
    skos:definition "Indiciates inclusion or applicability of a Third Party as a Recipient of persona data"@en ;
    skos:prefLabel "has recipient third party"@en ;
    schema:rangeIncludes dpv-owl:ThirdParty .

dpv-owl:hasRecordOfActivity a rdf:Property,
        owl:ObjectProperty ;
    dcam:rangeIncludes dpv-owl:RecordsOfActivities ;
    dct:contributor "Harshvardhan J. Pandit" ;
    dct:created "2024-05-05"^^xsd:date ;
    rdfs:isDefinedBy dpv-owl: ;
    rdfs:subPropertyOf dpv-owl:hasOrganisationalMeasure ;
    sw:term_status "accepted"@en ;
    skos:definition "Indicates a relevant record of activity"@en ;
    skos:prefLabel "has record of activity"@en ;
    schema:rangeIncludes dpv-owl:RecordsOfActivities .

dpv-owl:hasRelationWithDataSubject a rdf:Property,
        owl:ObjectProperty ;
    dcam:domainIncludes dpv-owl:Entity ;
    dct:contributor "Georg P. Krog, Harshvardhan J. Pandit, Paul Ryan, Julian Flake" ;
    dct:created "2022-06-21"^^xsd:date ;
    rdfs:isDefinedBy dpv-owl: ;
    rdfs:subPropertyOf dpv-owl:hasEntity ;
    sw:term_status "accepted"@en ;
    skos:definition "Indicates the relation between specified Entity and Data Subject"@en ;
    skos:prefLabel "has relation with data subject"@en ;
    schema:domainIncludes dpv-owl:Entity .

dpv-owl:hasRequestStatus a rdf:Property,
        owl:ObjectProperty ;
    dcam:rangeIncludes dpv-owl:RequestStatus ;
    dct:contributor "Harshvardhan J. Pandit" ;
    dct:created "2024-06-10"^^xsd:date ;
    rdfs:isDefinedBy dpv-owl: ;
    sw:term_status "accepted"@en ;
    skos:definition "Indicates the status associated with a request"@en ;
    skos:prefLabel "has request status"@en ;
    schema:rangeIncludes dpv-owl:RequestStatus .

dpv-owl:hasResidualRisk a rdf:Property,
        owl:ObjectProperty ;
    dcam:domainIncludes dpv-owl:Risk ;
    dcam:rangeIncludes dpv-owl:ResidualRisk ;
    dct:contributor "Harshvardhan J. Pandit, Georg P. Krog, Paul Ryan, Julian Flake" ;
    dct:created "2022-07-20"^^xsd:date ;
    vann:example dex-owl:E0068 ;
    rdfs:isDefinedBy dpv-owl: ;
    sw:term_status "accepted"@en ;
    skos:definition "Indicates the associated risk is the remaining or residual risk from applying mitigation measures or treatments to this risk"@en ;
    skos:prefLabel "has residual risk"@en ;
    schema:domainIncludes dpv-owl:Risk ;
    schema:rangeIncludes dpv-owl:ResidualRisk .

dpv-owl:hasResponsibleEntity a rdf:Property,
        owl:ObjectProperty ;
    dcam:rangeIncludes dpv-owl:Entity ;
    dct:contributor "Harshvardhan J. Pandit" ;
    dct:created "2022-03-02"^^xsd:date ;
    rdfs:isDefinedBy dpv-owl: ;
    rdfs:subPropertyOf dpv-owl:hasEntity ;
    sw:term_status "accepted"@en ;
    skos:definition "Specifies the indicated entity is responsible within some context"@en ;
    skos:prefLabel "has responsible entity"@en ;
    schema:rangeIncludes dpv-owl:Entity .

dpv-owl:hasRight a rdf:Property,
        owl:ObjectProperty ;
    dcam:rangeIncludes dpv-owl:Right ;
    dct:contributor "Harshvardhan J. Pandit" ;
    dct:created "2020-11-18"^^xsd:date ;
    vann:example dex-owl:E0061,
        dex-owl:E0067 ;
    rdfs:isDefinedBy dpv-owl: ;
    sw:term_status "accepted"@en ;
    skos:definition "Indicates use or applicability of Right"@en ;
    skos:prefLabel "has right"@en ;
    schema:rangeIncludes dpv-owl:Right .

dpv-owl:hasRisk a rdf:Property,
        owl:ObjectProperty ;
    dcam:rangeIncludes dpv-owl:Risk ;
    dct:contributor "Harshvardhan J. Pandit" ;
    dct:created "2020-11-18"^^xsd:date ;
    vann:example dex-owl:E0068 ;
    rdfs:isDefinedBy dpv-owl: ;
    sw:term_status "accepted"@en ;
    skos:definition "Indicates applicability of Risk for this concept"@en ;
    skos:prefLabel "has risk"@en ;
    schema:rangeIncludes dpv-owl:Risk .

dpv-owl:hasRiskAssessment a rdf:Property,
        owl:ObjectProperty ;
    dcam:rangeIncludes dpv-owl:RiskAssessment ;
    dct:contributor "Harshvardhan J. Pandit" ;
    dct:created "2024-04-14"^^xsd:date ;
    rdfs:isDefinedBy dpv-owl: ;
    rdfs:subPropertyOf dpv-owl:hasAssessment ;
    sw:term_status "accepted"@en ;
    skos:definition "Indicates an associated risk assessment"@en ;
    skos:prefLabel "has risk assessment"@en ;
    schema:rangeIncludes dpv-owl:RiskAssessment .

dpv-owl:hasRiskLevel a rdf:Property,
        owl:ObjectProperty ;
    dcam:domainIncludes dpv-owl:Risk ;
    dcam:rangeIncludes dpv-owl:RiskLevel ;
    dct:contributor "Harshvardhan J. Pandit, Georg P. Krog, Paul Ryan, Julian Flake" ;
    dct:created "2022-07-20"^^xsd:date ;
    vann:example dex-owl:E0068,
        dex-owl:E0071 ;
    rdfs:isDefinedBy dpv-owl: ;
    sw:term_status "accepted"@en ;
    skos:definition "Indicates the associated risk level associated with a risk"@en ;
    skos:prefLabel "has risk level"@en ;
    schema:domainIncludes dpv-owl:Risk ;
    schema:rangeIncludes dpv-owl:RiskLevel .

dpv-owl:hasScope a rdf:Property,
        owl:ObjectProperty ;
    dcam:rangeIncludes dpv-owl:Scope ;
    dct:contributor "Harshvardhan J. Pandit" ;
    dct:created "2022-06-15"^^xsd:date ;
    rdfs:isDefinedBy dpv-owl: ;
    sw:term_status "accepted"@en ;
    skos:definition "Indicates the scope of specified concept or context"@en ;
    skos:prefLabel "has scope"@en ;
    schema:rangeIncludes dpv-owl:Scope .

dpv-owl:hasSector a rdf:Property,
        owl:ObjectProperty ;
    dcam:rangeIncludes dpv-owl:Sector ;
    dct:created "2019-04-05"^^xsd:date ;
    rdfs:isDefinedBy dpv-owl: ;
    sw:term_status "accepted"@en ;
    skos:definition "Indicates the purpose is associated with activities in the indicated (Economic) Sector(s)"@en ;
    skos:prefLabel "has sector"@en ;
    schema:rangeIncludes dpv-owl:Sector .

dpv-owl:hasSensitivityLevel a rdf:Property,
        owl:ObjectProperty ;
    dcam:rangeIncludes dpv-owl:SensitivityLevel ;
    dct:contributor "Harshvardhan J. Pandit" ;
    dct:created "2023-08-24"^^xsd:date ;
    rdfs:isDefinedBy dpv-owl: ;
    sw:term_status "accepted"@en ;
    skos:definition "Indicates the associated level of sensitivity"@en ;
    skos:prefLabel "has sensitivity level"@en ;
    schema:rangeIncludes dpv-owl:SensitivityLevel .

dpv-owl:hasService a rdf:Property,
        owl:ObjectProperty ;
    dcam:rangeIncludes dpv-owl:Service ;
    dct:contributor "Harshvardhan J. Pandit" ;
    dct:created "2024-04-20"^^xsd:date ;
    rdfs:isDefinedBy dpv-owl: ;
    sw:term_status "accepted"@en ;
    skos:definition "Indicates associated with the specified service"@en ;
    skos:prefLabel "has service"@en ;
    schema:rangeIncludes dpv-owl:Service .

dpv-owl:hasServiceConsumer a rdf:Property,
        owl:ObjectProperty ;
    dcam:domainIncludes dpv-owl:Service ;
    dcam:rangeIncludes dpv-owl:ServiceConsumer ;
    dct:contributor "Harshvardhan J. Pandit" ;
    dct:created "2024-04-20"^^xsd:date ;
    rdfs:isDefinedBy dpv-owl: ;
    rdfs:subPropertyOf dpv-owl:hasEntity ;
    sw:term_status "accepted"@en ;
    skos:definition "Indicates the entity that consumes or receives the associated service"@en ;
    skos:prefLabel "has service consumer"@en ;
    schema:domainIncludes dpv-owl:Service ;
    schema:rangeIncludes dpv-owl:ServiceConsumer .

dpv-owl:hasServiceProvider a rdf:Property,
        owl:ObjectProperty ;
    dcam:domainIncludes dpv-owl:Service ;
    dcam:rangeIncludes dpv-owl:ServiceProvider ;
    dct:contributor "Harshvardhan J. Pandit" ;
    dct:created "2024-04-20"^^xsd:date ;
    rdfs:isDefinedBy dpv-owl: ;
    rdfs:subPropertyOf dpv-owl:hasEntity ;
    sw:term_status "accepted"@en ;
    skos:definition "Indicates the entity that provides the associated service"@en ;
    skos:prefLabel "has service provider"@en ;
    schema:domainIncludes dpv-owl:Service ;
    schema:rangeIncludes dpv-owl:ServiceProvider .

dpv-owl:hasSeverity a rdf:Property,
        owl:ObjectProperty ;
    dcam:rangeIncludes dpv-owl:Severity ;
    dct:contributor "Harshvardhan J. Pandit, Georg P. Krog, Paul Ryan, Julian Flake" ;
    dct:created "2022-07-20"^^xsd:date ;
    vann:example dex-owl:E0068 ;
    rdfs:isDefinedBy dpv-owl: ;
    sw:term_status "accepted"@en ;
    skos:definition "Indicates the severity associated with a concept"@en ;
    skos:prefLabel "has severity"@en ;
    schema:rangeIncludes dpv-owl:Severity .

dpv-owl:hasStorageCondition a rdf:Property,
        owl:ObjectProperty ;
    dcam:rangeIncludes dpv-owl:StorageCondition ;
    dct:contributor "Axel Polleres, Rob Brennan, Harshvardhan J. Pandit, Mark Lizar" ;
    dct:created "2022-08-13"^^xsd:date ;
    dct:source [ a schema:WebPage ;
            schema:name "SPECIAL Project" ;
            schema:url "https://specialprivacy.ercim.eu/" ] ;
    rdfs:isDefinedBy dpv-owl: ;
    rdfs:subPropertyOf dpv-owl:hasProcessingCondition ;
    sw:term_status "accepted"@en ;
    skos:definition "Indicates information about storage condition"@en ;
    skos:prefLabel "has storage condition"@en ;
    schema:rangeIncludes dpv-owl:StorageCondition .

dpv-owl:hasSubsidiary a rdf:Property,
        owl:ObjectProperty ;
    dcam:domainIncludes dpv-owl:Organisation ;
    dcam:rangeIncludes dpv-owl:Organisation ;
    dct:contributor "Harshvardhan J. Pandit, Georg P. Krog" ;
    dct:created "2024-04-14"^^xsd:date ;
    vann:example dex-owl:E0038 ;
    rdfs:isDefinedBy dpv-owl: ;
    rdfs:subPropertyOf dpv-owl:hasEntity ;
    sw:term_status "accepted"@en ;
    skos:definition "Indicates this entity has the specified entity as its subsidiary"@en ;
    skos:prefLabel "has subsidiary"@en ;
    schema:domainIncludes dpv-owl:Organisation ;
    schema:rangeIncludes dpv-owl:Organisation .

dpv-owl:hasTechnicalMeasure a rdf:Property,
        owl:ObjectProperty ;
    dcam:rangeIncludes dpv-owl:TechnicalMeasure ;
    dct:contributor "Harshvardhan J. Pandit" ;
    dct:created "2022-02-09"^^xsd:date ;
    vann:example dex-owl:E0064,
        dex-owl:E0070 ;
    rdfs:isDefinedBy dpv-owl: ;
    rdfs:subPropertyOf dpv-owl:hasTechnicalOrganisationalMeasure ;
    sw:term_status "accepted"@en ;
    skos:definition "Indicates use or applicability of Technical measure"@en ;
    skos:prefLabel "has technical measure"@en ;
    schema:rangeIncludes dpv-owl:TechnicalMeasure .

dpv-owl:hasThirdCountry a rdf:Property,
        owl:ObjectProperty ;
    dcam:rangeIncludes dpv-owl:ThirdCountry ;
    dct:contributor "Harshvardhan J. Pandit, Georg P. Krog" ;
    dct:created "2022-02-09"^^xsd:date ;
    rdfs:isDefinedBy dpv-owl: ;
    rdfs:subPropertyOf dpv-owl:hasCountry ;
    sw:term_status "accepted"@en ;
    skos:definition "Indicates applicability or relevance of a 'third country'"@en ;
    skos:prefLabel "has third country"@en ;
    schema:rangeIncludes dpv-owl:ThirdCountry .

dpv-owl:isAfter a rdf:Property,
        owl:ObjectProperty ;
    dcam:domainIncludes dpv-owl:RightExerciseActivity ;
    dcam:rangeIncludes dpv-owl:RightExerciseActivity ;
    dct:contributor "Georg P. Krog, Harshvardhan J. Pandit, Julian Flake" ;
    dct:created "2022-03-02"^^xsd:date ;
    rdfs:isDefinedBy dpv-owl: ;
    sw:term_status "accepted"@en ;
    skos:definition "Indicates the specified concepts is 'after' this concept in some context"@en ;
    skos:prefLabel "is after"@en ;
    skos:scopeNote "Also used for specifying a RightExerciseActivity occurs before another RightExerciseActivity"@en ;
    schema:domainIncludes dpv-owl:RightExerciseActivity ;
    schema:rangeIncludes dpv-owl:RightExerciseActivity .

dpv-owl:isApplicableFor a rdf:Property,
        owl:ObjectProperty ;
    dcam:rangeIncludes dpv-owl:Scope ;
    dct:contributor "Harshvardhan J. Pandit, Beatriz Esteves, Georg P. Krog, Paul Ryan" ;
    dct:created "2024-04-13"^^xsd:date ;
    rdfs:isDefinedBy dpv-owl: ;
    sw:term_status "accepted"@en ;
    skos:definition "Indicates the concept or information is applicable for specified context"@en ;
    skos:prefLabel "is applicable for"@en ;
    schema:rangeIncludes dpv-owl:Scope .

dpv-owl:isAuthorityFor a rdf:Property,
        owl:ObjectProperty ;
    dcam:domainIncludes dpv-owl:Authority ;
    dct:contributor "Harshvardhan J. Pandit, Georg P. Krog" ;
    dct:created "2022-01-19"^^xsd:date ;
    rdfs:isDefinedBy dpv-owl: ;
    sw:term_status "accepted"@en ;
    skos:definition "Indicates area, scope, or applicability of an Authority"@en ;
    skos:prefLabel "is authority for"@en ;
    schema:domainIncludes dpv-owl:Authority .

dpv-owl:isBefore a rdf:Property,
        owl:ObjectProperty ;
    dcam:domainIncludes dpv-owl:RightExerciseActivity ;
    dcam:rangeIncludes dpv-owl:RightExerciseActivity ;
    dct:contributor "Georg P. Krog, Harshvardhan J. Pandit, Julian Flake" ;
    dct:created "2022-03-02"^^xsd:date ;
    rdfs:isDefinedBy dpv-owl: ;
    sw:term_status "accepted"@en ;
    skos:definition "Indicates the specified concepts is 'before' this concept in some context"@en ;
    skos:prefLabel "is before"@en ;
    skos:scopeNote "Also used for specifying a RightExerciseActivity occurs before another RightExerciseActivity"@en ;
    schema:domainIncludes dpv-owl:RightExerciseActivity ;
    schema:rangeIncludes dpv-owl:RightExerciseActivity .

dpv-owl:isDeterminedByEntity a rdf:Property,
        owl:ObjectProperty ;
    dcam:rangeIncludes dpv-owl:Entity ;
    dct:contributor "Harshvardhan J. Pandit" ;
    dct:created "2024-05-10"^^xsd:date ;
    rdfs:isDefinedBy dpv-owl: ;
    rdfs:subPropertyOf dpv-owl:hasEntity ;
    sw:term_status "accepted"@en ;
    skos:definition "Indicates the context is determined by the specified entity"@en ;
    skos:prefLabel "is determined by entity"@en ;
    schema:rangeIncludes dpv-owl:Entity .

dpv-owl:isExercisedAt a rdf:Property,
        owl:ObjectProperty ;
    dcam:domainIncludes dpv-owl:ActiveRight ;
    dcam:rangeIncludes dpv-owl:RightExerciseNotice ;
    dct:contributor "Harshvardhan J. Pandit" ;
    dct:created "2022-10-22"^^xsd:date ;
    rdfs:isDefinedBy dpv-owl: ;
    sw:term_status "accepted"@en ;
    skos:definition "Indicates context or information about exercising a right"@en ;
    skos:prefLabel "is exercised at"@en ;
    schema:domainIncludes dpv-owl:ActiveRight ;
    schema:rangeIncludes dpv-owl:RightExerciseNotice .

dpv-owl:isImplementedByEntity a rdf:Property,
        owl:ObjectProperty ;
    dcam:domainIncludes dpv-owl:RightExerciseActivity ;
    dcam:rangeIncludes dpv-owl:Entity ;
    dct:contributor "Axel Polleres, Harshvardhan J. Pandit, Beatriz Esteves, Paul Ryan, Julian Flake" ;
    dct:created "2019-05-07"^^xsd:date ;
    dct:modified "2022-01-26"^^xsd:date ;
    vann:example dex-owl:E0037 ;
    rdfs:isDefinedBy dpv-owl: ;
    sw:term_status "accepted"@en ;
    skos:definition "Indicates implementation details such as entities or agents"@en ;
    skos:prefLabel "is implemented by entity"@en ;
    skos:scopeNote "Also used to indicate the Entity that implements or performs a Right Exercise Activity"@en,
        "The use of 'entity' is inclusive of entities (e.g. Data Processor) as well as 'agent' (e.g. DPO). For indicating technological implementation, the property isImplementedByTechnology should be used."@en ;
    schema:domainIncludes dpv-owl:RightExerciseActivity ;
    schema:rangeIncludes dpv-owl:Entity .

dpv-owl:isImplementedUsingTechnology a rdf:Property,
        owl:ObjectProperty ;
    dcam:rangeIncludes dpv-owl:Technology ;
    dct:contributor "Beatriz Esteves, Harshvardhan J. Pandit, Paul Ryan, Julian Flake" ;
    dct:created "2022-01-26"^^xsd:date ;
    dct:modified "2022-06-15"^^xsd:date ;
    vann:example dex-owl:E0064 ;
    rdfs:isDefinedBy dpv-owl: ;
    sw:term_status "accepted"@en ;
    skos:definition "Indicates implementation details such as technologies or processes"@en ;
    skos:prefLabel "is implemented using technology"@en ;
    skos:scopeNote "The term 'technology' is inclusive of technologies, processes, and methods."@en ;
    schema:rangeIncludes dpv-owl:Technology .

dpv-owl:isIndicatedAtTime a rdf:Property,
        owl:ObjectProperty ;
    dct:contributor "Georg P. Krog, Harshvardhan J. Pandit, Paul Ryan, Julian Flake" ;
    dct:created "2022-06-21"^^xsd:date ;
    rdfs:isDefinedBy dpv-owl: ;
    sw:term_status "accepted"@en ;
    skos:definition "Specifies the temporal information for when the entity has indicated the specific context"@en ;
    skos:prefLabel "is indicated at time"@en .

dpv-owl:isIndicatedBy a rdf:Property,
        owl:ObjectProperty ;
    dcam:rangeIncludes dpv-owl:Entity ;
    dct:contributor "Georg P. Krog, Harshvardhan J. Pandit, Paul Ryan, Julian Flake" ;
    dct:created "2022-06-21"^^xsd:date ;
    rdfs:isDefinedBy dpv-owl: ;
    sw:term_status "accepted"@en ;
    skos:definition "Specifies entity who indicates the specific context"@en ;
    skos:prefLabel "is indicated by"@en ;
    schema:rangeIncludes dpv-owl:Entity .

dpv-owl:isMitigatedByMeasure a rdf:Property,
        owl:ObjectProperty ;
    dcam:domainIncludes dpv-owl:Risk ;
    dcam:rangeIncludes dpv-owl:RiskMitigationMeasure ;
    dct:contributor "Harshvardhan J. Pandit" ;
    dct:created "2022-02-09"^^xsd:date ;
    vann:example dex-owl:E0068 ;
    rdfs:isDefinedBy dpv-owl: ;
    rdfs:subPropertyOf dpv-owl:hasTechnicalOrganisationalMeasure ;
    sw:term_status "accepted"@en ;
    skos:definition "Indicate a risk is mitigated by specified measure"@en ;
    skos:prefLabel "is mitigated by measure"@en ;
    schema:domainIncludes dpv-owl:Risk ;
    schema:rangeIncludes dpv-owl:RiskMitigationMeasure .

dpv-owl:isNotApplicableFor a rdf:Property,
        owl:ObjectProperty ;
    dcam:rangeIncludes dpv-owl:Scope ;
    dct:contributor "Harshvardhan J. Pandit, Beatriz Esteves, Georg P. Krog, Paul Ryan" ;
    dct:created "2024-04-13"^^xsd:date ;
    rdfs:isDefinedBy dpv-owl: ;
    sw:term_status "accepted"@en ;
    skos:definition "Indicates the concept or information is not applicable for specified context"@en ;
    skos:prefLabel "is not applicable for"@en ;
    schema:rangeIncludes dpv-owl:Scope .

dpv-owl:isOrganistionalUnitOf a rdf:Property,
        owl:ObjectProperty ;
    dcam:domainIncludes dpv-owl:OrganisationalUnit ;
    dcam:rangeIncludes dpv-owl:Entity ;
    dct:contributor "Harshvardhan J. Pandit" ;
    dct:created "2024-06-10"^^xsd:date ;
    rdfs:isDefinedBy dpv-owl: ;
    rdfs:subPropertyOf dpv-owl:hasEntity ;
    sw:term_status "accepted"@en ;
    skos:definition "Indicates this entity is an organisational unit of the specified entity"@en ;
    skos:prefLabel "is organisational unit of"@en ;
    schema:domainIncludes dpv-owl:OrganisationalUnit ;
    schema:rangeIncludes dpv-owl:Entity .

dpv-owl:isPolicyFor a rdf:Property,
        owl:ObjectProperty ;
    dcam:domainIncludes dpv-owl:Policy ;
    dct:contributor "Harshvardhan J. Pandit" ;
    dct:created "2022-01-26"^^xsd:date ;
    rdfs:isDefinedBy dpv-owl: ;
    sw:term_status "accepted"@en ;
    skos:definition "Indicates the context or application of policy"@en ;
    skos:prefLabel "is policy for"@en ;
    schema:domainIncludes dpv-owl:Policy .

dpv-owl:isRepresentativeFor a rdf:Property,
        owl:ObjectProperty ;
    dcam:domainIncludes dpv-owl:Representative ;
    dcam:rangeIncludes dpv-owl:Entity ;
    dct:contributor "Harshvardhan J. Pandit" ;
    dct:created "2022-11-09"^^xsd:date ;
    rdfs:isDefinedBy dpv-owl: ;
    rdfs:subPropertyOf dpv-owl:hasEntity ;
    sw:term_status "accepted"@en ;
    skos:definition "Indicates the entity is a representative for specified entity"@en ;
    skos:prefLabel "is representative for"@en ;
    schema:domainIncludes dpv-owl:Representative ;
    schema:rangeIncludes dpv-owl:Entity .

dpv-owl:isResidualRiskOf a rdf:Property,
        owl:ObjectProperty ;
    dcam:domainIncludes dpv-owl:ResidualRisk ;
    dcam:rangeIncludes dpv-owl:Risk ;
    dct:contributor "Harshvardhan J. Pandit, Georg P. Krog, Paul Ryan, Julian Flake" ;
    dct:created "2022-07-20"^^xsd:date ;
    rdfs:isDefinedBy dpv-owl: ;
    sw:term_status "accepted"@en ;
    skos:definition "Indicates this risk is the remaining or residual risk from applying mitigation measures or treatments to specified risk"@en ;
    skos:prefLabel "is residual risk of"@en ;
    schema:domainIncludes dpv-owl:ResidualRisk ;
    schema:rangeIncludes dpv-owl:Risk .

dpv-owl:isSubsidiaryOf a rdf:Property,
        owl:ObjectProperty ;
    dcam:domainIncludes dpv-owl:Organisation ;
    dcam:rangeIncludes dpv-owl:Organisation ;
    dct:contributor "Harshvardhan J. Pandit, Georg P. Krog" ;
    dct:created "2024-04-14"^^xsd:date ;
    rdfs:isDefinedBy dpv-owl: ;
    rdfs:subPropertyOf dpv-owl:hasEntity ;
    sw:term_status "accepted"@en ;
    skos:definition "Indicates this entity is the subsidiary of the specified entity"@en ;
    skos:prefLabel "is subsidiary of"@en ;
    schema:domainIncludes dpv-owl:Organisation ;
    schema:rangeIncludes dpv-owl:Organisation .

dpv-owl:mitigatesRisk a rdf:Property,
        owl:ObjectProperty ;
    dcam:domainIncludes dpv-owl:RiskMitigationMeasure ;
    dcam:rangeIncludes dpv-owl:Risk ;
    dct:contributor "Harshvardhan J. Pandit" ;
    dct:created "2020-11-04"^^xsd:date ;
    rdfs:isDefinedBy dpv-owl: ;
    sw:term_status "accepted"@en ;
    skos:definition "Indicates risks mitigated by this concept"@en ;
    skos:prefLabel "mitigates risk"@en ;
    schema:domainIncludes dpv-owl:RiskMitigationMeasure ;
    schema:rangeIncludes dpv-owl:Risk .

dpv-owl:supportsComplianceWith a rdf:Property,
        owl:ObjectProperty ;
    dcam:domainIncludes dpv-owl:TechnicalOrganisationalMeasure ;
    dct:contributor "Julian Flake, Georg P. Krog, Harshvardhan J. Pandit" ;
    dct:created "2024-04-14"^^xsd:date ;
    rdfs:isDefinedBy dpv-owl: ;
    sw:term_status "accepted"@en ;
    skos:definition "Indicate the measure is required for meeting specified requirement or satisfying specified condition/constraint"@en ;
    skos:prefLabel "supports Compliance With"@en ;
    schema:domainIncludes dpv-owl:TechnicalOrganisationalMeasure .

dpv-owl:hasComplianceStatus a rdf:Property,
        owl:ObjectProperty ;
    dcam:rangeIncludes dpv-owl:ComplianceStatus ;
    dct:contributor "Harshvardhan J. Pandit" ;
    dct:created "2022-05-18"^^xsd:date ;
    vann:example dex-owl:E0055 ;
    rdfs:isDefinedBy dpv-owl: ;
    rdfs:subPropertyOf dpv-owl:hasStatus ;
    sw:term_status "accepted"@en ;
    skos:definition "Indicates the status of compliance of specified concept"@en ;
    skos:prefLabel "has compliance status"@en ;
    schema:rangeIncludes dpv-owl:ComplianceStatus .

dpv-owl:hasConsequence a rdf:Property,
        owl:ObjectProperty ;
    dcam:rangeIncludes dpv-owl:Consequence ;
    dct:contributor "Harshvardhan J. Pandit, Julian Flake, Georg P. Krog, Fajar Ekaputra, Beatriz Esteves" ;
    dct:created "2020-11-04"^^xsd:date ;
    dct:modified "2021-09-21"^^xsd:date ;
    vann:example dex-owl:E0068,
        dex-owl:E0071 ;
    rdfs:isDefinedBy dpv-owl: ;
    sw:term_status "accepted"@en ;
    skos:definition "Indicates consequence(s) possible or arising from specified concept"@en ;
    skos:prefLabel "has consequence"@en ;
    skos:scopeNote "Removed plural suffix for consistency"@en ;
    schema:rangeIncludes dpv-owl:Consequence .

dpv-owl:hasConsequenceOn a rdf:Property,
        owl:ObjectProperty ;
    dcam:domainIncludes dpv-owl:Consequence ;
    dct:contributor "Harshvardhan J. Pandit, Georg P. Krog" ;
    dct:created "2022-11-24"^^xsd:date ;
    rdfs:isDefinedBy dpv-owl: ;
    sw:term_status "accepted"@en ;
    skos:definition "Indicates the thing (e.g. plan, process, or entity) affected by a consequence"@en ;
    skos:prefLabel "has consequence on"@en ;
    schema:domainIncludes dpv-owl:Consequence .

dpv-owl:hasCountry a rdf:Property,
        owl:ObjectProperty ;
    dcam:rangeIncludes dpv-owl:Country ;
    dct:contributor "Harshvardhan J. Pandit, Georg P. Krog" ;
    dct:created "2022-01-19"^^xsd:date ;
    rdfs:isDefinedBy dpv-owl: ;
    rdfs:subPropertyOf dpv-owl:hasLocation ;
    sw:term_status "accepted"@en ;
    skos:definition "Indicates applicability of specified country"@en ;
    skos:prefLabel "has country"@en ;
    schema:rangeIncludes dpv-owl:Country .

dpv-owl:hasData a rdf:Property,
        owl:ObjectProperty ;
    dcam:rangeIncludes dpv-owl:Data ;
    dct:contributor "Harshvardhan J. Pandit" ;
    dct:created "2022-08-18"^^xsd:date ;
    rdfs:isDefinedBy dpv-owl: ;
    sw:term_status "accepted"@en ;
    skos:definition "Indicates associated with Data (may or may not be personal)"@en ;
    skos:prefLabel "has data"@en ;
    schema:rangeIncludes dpv-owl:Data .

dpv-owl:hasDataController a rdf:Property,
        owl:ObjectProperty ;
    dcam:rangeIncludes dpv-owl:DataController ;
    dct:contributor "Axel Polleres, Javier Fernández, Harshvardhan J. Pandit, Mark Lizar, Bud Bruegger" ;
    dct:created "2019-04-04"^^xsd:date ;
    dct:modified "2020-11-04"^^xsd:date ;
    rdfs:isDefinedBy dpv-owl: ;
    rdfs:subPropertyOf dpv-owl:hasEntity ;
    sw:term_status "accepted"@en ;
    skos:definition "Indicates association with Data Controller"@en ;
    skos:prefLabel "has data controller"@en ;
    schema:rangeIncludes dpv-owl:DataController .

dpv-owl:hasLocation a rdf:Property,
        owl:ObjectProperty ;
    dcam:rangeIncludes dpv-owl:Location ;
    dct:contributor "Axel Polleres, Rob Brennan, Harshvardhan J. Pandit, Mark Lizar" ;
    dct:created "2019-04-05"^^xsd:date ;
    dct:source [ a schema:WebPage ;
            schema:name "SPECIAL Project" ;
            schema:url "https://specialprivacy.ercim.eu/" ] ;
    vann:example dex-owl:E0060 ;
    rdfs:isDefinedBy dpv-owl: ;
    sw:term_status "accepted"@en ;
    skos:definition "Indicates information about location"@en ;
    skos:prefLabel "has location"@en ;
    schema:rangeIncludes dpv-owl:Location .

dpv-owl:hasProcessingCondition a rdf:Property,
        owl:ObjectProperty ;
    dcam:rangeIncludes dpv-owl:ProcessingCondition ;
    dct:contributor "Harshvardhan J. Pandit" ;
    dct:created "2023-12-10"^^xsd:date ;
    rdfs:isDefinedBy dpv-owl: ;
    sw:term_status "accepted"@en ;
    skos:definition "Indicates information about processing condition"@en ;
    skos:prefLabel "has processing condition"@en ;
    schema:rangeIncludes dpv-owl:ProcessingCondition .

dpv-owl:hasRepresentative a rdf:Property,
        owl:ObjectProperty ;
    dcam:domainIncludes dpv-owl:Entity ;
    dcam:rangeIncludes dpv-owl:Representative ;
    dct:contributor "Harshvardhan J. Pandit, Georg P. Krog, Paul Ryan, Beatriz Esteves" ;
    dct:created "2020-11-04"^^xsd:date ;
    rdfs:isDefinedBy dpv-owl: ;
    rdfs:subPropertyOf dpv-owl:hasEntity ;
    sw:term_status "accepted"@en ;
    skos:definition "Specifies representative of the legal entity"@en ;
    skos:prefLabel "has representative"@en ;
    schema:domainIncludes dpv-owl:Entity ;
    schema:rangeIncludes dpv-owl:Representative .

dpv-owl:serialisation-html a profile:ResourceDescriptor ;
    dct:conformsTo <https://www.w3.org/TR/html/> ;
    dct:format <https://www.iana.org/assignments/media-types/text/html> ;
    dct:title "Data Privacy Vocabulary (DPV) - HTML serialiation" ;
    profile:hasArtifact <https://w3id.org/dpv/dpv-owl.html> ;
    profile:hasRole role:specification .

dpv-owl:serialisation-jsonld a profile:ResourceDescriptor ;
    dct:conformsTo <https://www.w3.org/TR/json-ld11/> ;
    dct:format <https://www.iana.org/assignments/media-types/application/ld+json> ;
    dct:title "Data Privacy Vocabulary (DPV) - JSON-LD serialiation" ;
    profile:hasArtifact <https://w3id.org/dpv/dpv/dpv-owl.jsonld> ;
    profile:hasRole role:vocabulary .

dpv-owl:serialisation-n3 a profile:ResourceDescriptor ;
    dct:conformsTo <https://www.w3.org/TeamSubmission/n3/> ;
    dct:format <https://www.iana.org/assignments/media-types/text/n3> ;
    dct:title "Data Privacy Vocabulary (DPV) - N3 serialiation" ;
    profile:hasArtifact <https://w3id.org/dpv/dpv/dpv-owl.n3> ;
    profile:hasRole role:vocabulary .

dpv-owl:serialisation-rdf a profile:ResourceDescriptor ;
    dct:conformsTo rdf: ;
    dct:format <https://www.iana.org/assignments/media-types/application/rdf+xml> ;
    dct:title "Data Privacy Vocabulary (DPV) - RDF/XML serialiation" ;
    profile:hasArtifact <https://w3id.org/dpv/dpv/dpv-owl.rdf> ;
    profile:hasRole role:vocabulary .

dpv-owl:serialisation-ttl a profile:ResourceDescriptor ;
    dct:conformsTo <https://www.w3.org/TR/turtle/> ;
    dct:format <https://www.iana.org/assignments/media-types/text/turtle> ;
    dct:title "Data Privacy Vocabulary (DPV) - Turtle serialiation" ;
    profile:hasArtifact <https://w3id.org/dpv/dpv/dpv-owl.ttl> ;
    profile:hasRole role:vocabulary .

<https://w3id.org/dpv/examples> a profile:ResourceDescriptor ;
    dct:conformsTo <https://www.w3.org/TR/html/> ;
    dct:format <https://www.iana.org/assignments/media-types/text/html> ;
    dct:title "Examples for Data Privacy Vocabulary" ;
    profile:hasArtifact <https://w3id.org/dpv/examples> ;
    profile:hasRole role:guidance .

<https://w3id.org/dpv/guides> a profile:ResourceDescriptor ;
    dct:conformsTo <https://www.w3.org/TR/html/> ;
    dct:format <https://www.iana.org/assignments/media-types/text/html> ;
    dct:title "Guides for Data Privacy Vocabulary" ;
    profile:hasArtifact <https://w3id.org/dpv/guides> ;
    profile:hasRole role:guidance .

dpv-owl:hasAssessment a rdf:Property,
        owl:ObjectProperty ;
    dcam:rangeIncludes dpv-owl:Assessment ;
    dct:contributor "Harshvardhan J. Pandit" ;
    dct:created "2024-04-14"^^xsd:date ;
    rdfs:isDefinedBy dpv-owl: ;
    rdfs:subPropertyOf dpv-owl:hasOrganisationalMeasure ;
    sw:term_status "accepted"@en ;
    skos:definition "Indicates a relevant assessment associated with the specific context"@en ;
    skos:prefLabel "has assessment"@en ;
    schema:rangeIncludes dpv-owl:Assessment .

<https://w3id.org/dpv/primer> a profile:ResourceDescriptor ;
    dct:conformsTo <https://www.w3.org/TR/html/> ;
    dct:format <https://www.iana.org/assignments/media-types/text/html> ;
    dct:title "Primer for Data Privacy Vocabulary" ;
    profile:hasArtifact <https://w3id.org/dpv/primer> ;
    profile:hasRole role:guidance .

dpv-owl:hasRule a rdf:Property,
        owl:ObjectProperty ;
    dcam:domainIncludes dpv-owl:Context ;
    dcam:rangeIncludes dpv-owl:Rule ;
    dct:contributor "Harshvardhan J. Pandit, Georg P. Krog, Beatriz Esteves, Paul Ryan" ;
    dct:created "2022-10-19"^^xsd:date ;
    rdfs:isDefinedBy dpv-owl: ;
    sw:term_status "accepted"@en ;
    skos:definition "Specifying applicability or inclusion of a rule within specified context"@en ;
    skos:prefLabel "has rule"@en ;
    schema:domainIncludes dpv-owl:Context ;
    schema:rangeIncludes dpv-owl:Rule .

dpv-owl:hasScale a rdf:Property,
        owl:ObjectProperty ;
    dcam:rangeIncludes dpv-owl:Scale ;
    dct:contributor "Harshvardhan J. Pandit" ;
    dct:created "2022-06-15"^^xsd:date ;
    rdfs:isDefinedBy dpv-owl: ;
    sw:term_status "accepted"@en ;
    skos:definition "Indicates the scale of specified concept"@en ;
    skos:prefLabel "has scale"@en ;
    schema:rangeIncludes dpv-owl:Scale .

dpv-owl:hasOrganisationalMeasure a rdf:Property,
        owl:ObjectProperty ;
    dcam:rangeIncludes dpv-owl:OrganisationalMeasure ;
    dct:contributor "Harshvardhan J. Pandit" ;
    dct:created "2022-02-09"^^xsd:date ;
    rdfs:isDefinedBy dpv-owl: ;
    rdfs:subPropertyOf dpv-owl:hasTechnicalOrganisationalMeasure ;
    sw:term_status "accepted"@en ;
    skos:definition "Indicates use or applicability of Organisational measure"@en ;
    skos:prefLabel "has organisational measure"@en ;
    schema:rangeIncludes dpv-owl:OrganisationalMeasure .

dpv-owl:hasRecipient a rdf:Property,
        owl:ObjectProperty ;
    dcam:domainIncludes dpv-owl:RightExerciseActivity ;
    dcam:rangeIncludes dpv-owl:Recipient ;
    dct:contributor "Axel Polleres, Javier Fernández, Harshvardhan J. Pandit, Mark Lizar, Bud Bruegger" ;
    dct:created "2019-04-04"^^xsd:date ;
    dct:modified "2020-11-04"^^xsd:date ;
    dct:source [ a schema:WebPage ;
            schema:name "SPECIAL Project" ;
            schema:url "https://specialprivacy.ercim.eu/" ] ;
    rdfs:isDefinedBy dpv-owl: ;
    rdfs:subPropertyOf dpv-owl:hasEntity ;
    sw:term_status "accepted"@en ;
    skos:definition "Indicates Recipient of Data"@en ;
    skos:prefLabel "has recipient"@en ;
    skos:scopeNote "Also used to indicate the Recipient of a Right Exercise Activity"@en ;
    schema:domainIncludes dpv-owl:RightExerciseActivity ;
    schema:rangeIncludes dpv-owl:Recipient .

dpv-owl:hasTechnicalOrganisationalMeasure a rdf:Property,
        owl:ObjectProperty ;
    dcam:rangeIncludes dpv-owl:TechnicalOrganisationalMeasure ;
    dct:contributor "Axel Polleres, Javier Fernández, Harshvardhan J. Pandit, Mark Lizar, Bud Bruegger" ;
    dct:created "2019-04-04"^^xsd:date ;
    dct:modified "2020-11-04"^^xsd:date ;
    rdfs:isDefinedBy dpv-owl: ;
    sw:term_status "accepted"@en ;
    skos:definition "Indicates use or applicability of Technical or Organisational measure"@en ;
    skos:prefLabel "has technical and organisational measure"@en ;
    schema:rangeIncludes dpv-owl:TechnicalOrganisationalMeasure .

dpv-owl:hasStatus a rdf:Property,
        owl:ObjectProperty ;
    dcam:domainIncludes dpv-owl:RightExerciseActivity ;
    dcam:rangeIncludes dpv-owl:Status ;
    dct:contributor "Harshvardhan J. Pandit" ;
    dct:created "2022-05-18"^^xsd:date ;
    vann:example dex-owl:E0069 ;
    rdfs:isDefinedBy dpv-owl: ;
    sw:term_status "accepted"@en ;
    skos:definition "Indicates the status of specified concept"@en ;
    skos:prefLabel "has status"@en ;
    skos:scopeNote "Also used to Indicate the status of a Right Exercise Activity"@en ;
    schema:domainIncludes dpv-owl:RightExerciseActivity ;
    schema:rangeIncludes dpv-owl:Status .

dpv-owl:hasEntity a rdf:Property,
        owl:ObjectProperty ;
    dcam:rangeIncludes dpv-owl:Entity ;
    dct:contributor "Harshvardhan J. Pandit" ;
    dct:created "2022-02-09"^^xsd:date ;
    rdfs:isDefinedBy dpv-owl: ;
    sw:term_status "accepted"@en ;
    skos:definition "Indicates inclusion or applicability of an entity to some concept"@en ;
    skos:prefLabel "has entity"@en ;
    skos:scopeNote "parent property for controller, processor, data subject, authority, etc.?"@en ;
    schema:rangeIncludes dpv-owl:Entity .

dpv-owl: a owl:Ontology,
        profile:Profile ;
    dct:bibliographicCitation "Data Privacy Vocabulary (DPV) -- Version 2. Harshvardhan J. Pandit, Beatriz Esteves, Georg P. Krog, Paul Ryan, Delaram Golpayegani, Julian Flake https://doi.org/10.48550/arXiv.2404.13426" ;
    dct:conformsTo <http://www.w3.org/2002/07/owl>,
        "http://www.w3.org/2000/01/rdf-schema",
        "http://www.w3.org/2004/02/skos/core" ;
    dct:contributor "Arthit Suriyawongkul",
        "Axel Polleres",
        "Beatriz Esteves",
        "Bud Bruegger",
        "Damien Desfontaines",
        "David Hickey",
        "Delaram Golpayegani",
        "Elmar Kiesling",
        "Fajar Ekaputra",
        "Georg P. Krog",
        "Harshvardhan J. Pandit",
        "Javier Fernández",
        "Julian Flake",
        "Mark Lizar",
        "Maya Borges",
        "Paul Ryan",
        "Piero Bonatti",
        "Rana Saniei",
        "Rob Brennan",
        "Rudy Jacob",
        "Simon Steyskal",
        "Steve Hickman" ;
    dct:created "2022-08-18"@en ;
    dct:creator "Beatriz Esteves"@en,
        "Delaram Golpayegani"@en,
        "Georg P. Krog"@en,
        "Harshvardhan J. Pandit"@en,
        "Julian Flake"@en,
        "Paul Ryan"@en ;
    dct:description "The Data Privacy Vocabulary (DPV) provides terms (classes and properties) to represent information about processing of personal data, for example - purposes, processing operations, personal data, technical and organisational measures."@en ;
    dct:hasVersion dpv-owl: ;
    dct:identifier "https://w3id.org/dpv" ;
    dct:issued "2022-08-18"@en ;
    dct:license <https://www.w3.org/copyright/document-license-2023/> ;
    dct:modified "2024-07-01"@en ;
    dct:publisher <https://www.w3.org/> ;
    dct:source <https://www.w3.org/groups/cg/dpvcg/> ;
    dct:title "Data Privacy Vocabulary (DPV)"@en ;
    bibo:doi "10.5281/zenodo.12505841" ;
    bibo:status "http://purl.org/ontology/bibo/status/published" ;
    vann:preferredNamespacePrefix "dpv" ;
    vann:preferredNamespaceUri "https://w3id.org/dpv#" ;
    rdfs:Label "DPV"@en ;
    owl:versionIRI <https://w3id.org/dpv/2.0/owl#> ;
    owl:versionInfo "2.0" ;
    profile:hasResource <https://w3id.org/dpv/examples>,
        <https://w3id.org/dpv/guides>,
        dpv-owl:serialisation-html,
        dpv-owl:serialisation-jsonld,
        dpv-owl:serialisation-n3,
        dpv-owl:serialisation-rdf,
        dpv-owl:serialisation-ttl,
        <https://w3id.org/dpv/primer> ;
    profile:isProfileOf <http://www.w3.org/2002/07/owl>,
        dpv-owl: ;
    foaf:logo <https://w3id.org/dpv/media/logo.png> ;
    schema:version "2.0" .

