@prefix ai-owl: <https://w3id.org/dpv/ai/owl#> .
@prefix bibo: <http://purl.org/ontology/bibo/> .
@prefix dct: <http://purl.org/dc/terms/> .
@prefix dpv-owl: <https://w3id.org/dpv/owl#> .
@prefix foaf: <http://xmlns.com/foaf/0.1/> .
@prefix org: <http://www.w3.org/ns/org#> .
@prefix owl: <http://www.w3.org/2002/07/owl#> .
@prefix profile: <http://www.w3.org/ns/dx/prof/> .
@prefix rdf: <http://www.w3.org/1999/02/22-rdf-syntax-ns#> .
@prefix rdfs: <http://www.w3.org/2000/01/rdf-schema#> .
@prefix role: <http://www.w3.org/ns/dx/prof/role/> .
@prefix schema: <https://schema.org/> .
@prefix scoro: <http://purl.org/spar/scoro/> .
@prefix skos: <http://www.w3.org/2004/02/skos/core#> .
@prefix sw: <http://www.w3.org/2003/06/sw-vocab-status/ns#> .
@prefix tech-owl: <https://w3id.org/dpv/tech/owl#> .
@prefix vann: <http://purl.org/vocab/vann/> .
@prefix xsd: <http://www.w3.org/2001/XMLSchema#> .

ai-owl:AGI a rdfs:Class,
        owl:Class ;
    dct:contributor _:Ne8d6151e3d8047e6a947b3ec1a3830a1 ;
    dct:created "2024-12-01"^^xsd:date ;
    dct:source "ISO/IEC 22989:2022"@en ;
    rdfs:isDefinedBy ai-owl: ;
    rdfs:subClassOf ai-owl:AISystem ;
    sw:term_status "accepted"@en ;
    skos:definition "Type of AI system that addresses a broad range of tasks with a satisfactory level of performance"@en ;
    skos:prefLabel "Artificial General Intelligence (AGI)"@en .

ai-owl:CognitiveComputing a rdfs:Class,
        owl:Class ;
    dct:contributor _:Ne8d6151e3d8047e6a947b3ec1a3830a1 ;
    dct:created "2024-12-01"^^xsd:date ;
    dct:source " 3.1.8"@en,
        "ISO/IEC 22989:2022"@en ;
    rdfs:isDefinedBy ai-owl: ;
    rdfs:subClassOf ai-owl:AISystem ;
    sw:term_status "accepted"@en ;
    skos:definition "Category of AI systems that enables people and machines to interact more naturally"@en ;
    skos:prefLabel "Cognitive Computing"@en .

ai-owl:ExpertSystem a rdfs:Class,
        owl:Class ;
    dct:contributor _:Ne8d6151e3d8047e6a947b3ec1a3830a1 ;
    dct:created "2024-12-01"^^xsd:date ;
    dct:source " 3.1.13"@en,
        "ISO/IEC 22989:2022"@en ;
    rdfs:isDefinedBy ai-owl: ;
    rdfs:subClassOf ai-owl:AISystem ;
    sw:term_status "accepted"@en ;
    skos:definition "AI system that accumulates, combines and encapsulates knowledge provided by a human expert or experts in a specific domain to infer solutions to problems"@en ;
    skos:prefLabel "Expert System"@en .

ai-owl:GPAIModel a rdfs:Class,
        owl:Class ;
    dct:contributor _:Ne8d6151e3d8047e6a947b3ec1a3830a1 ;
    dct:created "2024-12-01"^^xsd:date ;
    dct:source "EU AI Act"@en ;
    rdfs:isDefinedBy ai-owl: ;
    rdfs:subClassOf ai-owl:Model ;
    sw:term_status "accepted"@en ;
    skos:definition "A model that displays generality in terms of capabilities and potential applications"@en ;
    skos:prefLabel "General Purpose AI Model"@en .

ai-owl:IndustrialRobot a rdfs:Class,
        owl:Class ;
    dct:contributor _:Ne8d6151e3d8047e6a947b3ec1a3830a1 ;
    dct:created "2024-12-01"^^xsd:date ;
    dct:source " 3.1.29"@en,
        "ISO/IEC 22989:2022"@en ;
    rdfs:isDefinedBy ai-owl: ;
    rdfs:subClassOf ai-owl:Robot ;
    sw:term_status "accepted"@en ;
    skos:definition "A robot or robotic system for use in industrial automation applications"@en ;
    skos:prefLabel "Industrial Robot"@en .

ai-owl:IntelligentControlSystem a rdfs:Class,
        owl:Class ;
    dct:contributor _:Ne8d6151e3d8047e6a947b3ec1a3830a1 ;
    dct:created "2024-12-01"^^xsd:date ;
    dct:source " Defining Artificial Intelligence 2.0"@en,
        "AI Watch"@en ;
    rdfs:isDefinedBy ai-owl: ;
    rdfs:subClassOf ai-owl:AISystem ;
    sw:term_status "accepted"@en ;
    skos:definition "Category of AI systems which implement intelligent control principles for real-world applications by using AI capabilities and techniques"@en ;
    skos:prefLabel "Intelligent Control System"@en .

ai-owl:MachineLearningModel a rdfs:Class,
        owl:Class ;
    dct:contributor _:Ne8d6151e3d8047e6a947b3ec1a3830a1 ;
    dct:created "2024-12-01"^^xsd:date ;
    dct:source " 3.3.7"@en,
        "ISO/IEC 22989:2022"@en ;
    rdfs:isDefinedBy ai-owl: ;
    rdfs:subClassOf ai-owl:Model ;
    sw:term_status "accepted"@en ;
    skos:definition "Mathematical construct that generates an inference or prediction  based on input data or information"@en ;
    skos:prefLabel "Machine Learning Model"@en .

ai-owl:MachineLearningPlatform a rdfs:Class,
        owl:Class,
        dpv-owl:Technology ;
    dct:contributor _:Ne8d6151e3d8047e6a947b3ec1a3830a1 ;
    dct:created "2024-12-01"^^xsd:date ;
    rdfs:isDefinedBy ai-owl: ;
    rdfs:subClassOf tech-owl:Platform ;
    sw:term_status "accepted"@en ;
    skos:definition "Technology platform for developing, deploying, and managing machine learning models and resources"@en ;
    skos:prefLabel "Machine Learning Platform"@en .

ai-owl:NarrowAI a rdfs:Class,
        owl:Class ;
    dct:contributor _:Ne8d6151e3d8047e6a947b3ec1a3830a1 ;
    dct:created "2024-12-01"^^xsd:date ;
    dct:source " 3.1.24"@en,
        "ISO/IEC 22989:2022"@en ;
    rdfs:isDefinedBy ai-owl: ;
    rdfs:subClassOf ai-owl:AISystem ;
    sw:term_status "accepted"@en ;
    skos:definition "Type of AI system that is focused on defined tasks to address a specific problem i.e. it addresses a narrow scope of tasks and problems"@en ;
    skos:prefLabel "Narrow AI"@en .

ai-owl:Robot a rdfs:Class,
        owl:Class ;
    dct:contributor _:Ne8d6151e3d8047e6a947b3ec1a3830a1 ;
    dct:created "2024-12-01"^^xsd:date ;
    dct:source " 3.1.29"@en,
        "ISO/IEC 22989:2022"@en ;
    rdfs:isDefinedBy ai-owl: ;
    rdfs:subClassOf ai-owl:AISystem ;
    sw:term_status "accepted"@en ;
    skos:definition "An automation system with actuators that performs intended tasks in the physical world, by means of sensing its environment and a software control system"@en ;
    skos:prefLabel "Robot"@en .

ai-owl:ServiceRobot a rdfs:Class,
        owl:Class ;
    dct:contributor _:Ne8d6151e3d8047e6a947b3ec1a3830a1 ;
    dct:created "2024-12-01"^^xsd:date ;
    dct:source " 3.1.29"@en,
        " 3.7"@en,
        " ISO 8373:2021"@en,
        "ISO/IEC 22989:2022"@en ;
    rdfs:isDefinedBy ai-owl: ;
    rdfs:subClassOf ai-owl:Robot ;
    sw:term_status "accepted"@en ;
    skos:definition "A robot or robotic system in personal use or professional use that performs useful tasks for humans or equipment"@en ;
    skos:prefLabel "Service Robot"@en .

ai-owl:SocialRobot a rdfs:Class,
        owl:Class ;
    dct:contributor _:Ne8d6151e3d8047e6a947b3ec1a3830a1 ;
    dct:created "2024-12-01"^^xsd:date ;
    dct:source " Defining Artificial Intelligence 2.0"@en,
        "AI Watch"@en ;
    rdfs:isDefinedBy ai-owl: ;
    rdfs:subClassOf ai-owl:Robot ;
    sw:term_status "accepted"@en ;
    skos:definition "A robot or robotic system with social interaction functions"@en ;
    skos:prefLabel "Social Robot"@en .

ai-owl:TrainedModel a rdfs:Class,
        owl:Class ;
    dct:contributor _:Ne8d6151e3d8047e6a947b3ec1a3830a1 ;
    dct:created "2024-12-01"^^xsd:date ;
    dct:source " 3.3.14"@en,
        "ISO/IEC 22989:2022"@en ;
    rdfs:isDefinedBy ai-owl: ;
    rdfs:subClassOf ai-owl:Model ;
    sw:term_status "accepted"@en ;
    skos:definition "Model resulted from model training"@en ;
    skos:prefLabel "Trained Model"@en .

ai-owl:serialisation-html a profile:ResourceDescriptor ;
    dct:conformsTo <https://www.w3.org/TR/html/> ;
    dct:format <https://www.iana.org/assignments/media-types/text/html> ;
    dct:title "AI Technology Concepts - HTML serialiation" ;
    profile:hasArtifact <https://w3id.org/dpv/ai/ai-owl.html> ;
    profile:hasRole role:specification .

ai-owl:serialisation-jsonld a profile:ResourceDescriptor ;
    dct:conformsTo <https://www.w3.org/TR/json-ld11/> ;
    dct:format <https://www.iana.org/assignments/media-types/application/ld+json> ;
    dct:title "AI Technology Concepts - JSON-LD serialiation" ;
    profile:hasArtifact <https://w3id.org/dpv/ai/ai-owl.jsonld> ;
    profile:hasRole role:vocabulary .

ai-owl:serialisation-n3 a profile:ResourceDescriptor ;
    dct:conformsTo <https://www.w3.org/TeamSubmission/n3/> ;
    dct:format <https://www.iana.org/assignments/media-types/text/n3> ;
    dct:title "AI Technology Concepts - N3 serialiation" ;
    profile:hasArtifact <https://w3id.org/dpv/ai/ai-owl.n3> ;
    profile:hasRole role:vocabulary .

ai-owl:serialisation-rdf a profile:ResourceDescriptor ;
    dct:conformsTo rdf: ;
    dct:format <https://www.iana.org/assignments/media-types/application/rdf+xml> ;
    dct:title "AI Technology Concepts - RDF/XML serialiation" ;
    profile:hasArtifact <https://w3id.org/dpv/ai/ai-owl.rdf> ;
    profile:hasRole role:vocabulary .

ai-owl:serialisation-ttl a profile:ResourceDescriptor ;
    dct:conformsTo <https://www.w3.org/TR/turtle/> ;
    dct:format <https://www.iana.org/assignments/media-types/text/turtle> ;
    dct:title "AI Technology Concepts - Turtle serialiation" ;
    profile:hasArtifact <https://w3id.org/dpv/ai/ai-owl.ttl> ;
    profile:hasRole role:vocabulary .

<https://w3id.org/dpv/examples> a profile:ResourceDescriptor ;
    dct:conformsTo <https://www.w3.org/TR/html/> ;
    dct:format <https://www.iana.org/assignments/media-types/text/html> ;
    dct:title "Examples for Data Privacy Vocabulary" ;
    profile:hasArtifact <https://w3id.org/dpv/examples> ;
    profile:hasRole role:guidance .

<https://w3id.org/dpv/guides> a profile:ResourceDescriptor ;
    dct:conformsTo <https://www.w3.org/TR/html/> ;
    dct:format <https://www.iana.org/assignments/media-types/text/html> ;
    dct:title "Guides for Data Privacy Vocabulary" ;
    profile:hasArtifact <https://w3id.org/dpv/guides> ;
    profile:hasRole role:guidance .

<https://w3id.org/dpv/primer> a profile:ResourceDescriptor ;
    dct:conformsTo <https://www.w3.org/TR/html/> ;
    dct:format <https://www.iana.org/assignments/media-types/text/html> ;
    dct:title "Primer for Data Privacy Vocabulary" ;
    profile:hasArtifact <https://w3id.org/dpv/primer> ;
    profile:hasRole role:guidance .

ai-owl: a owl:Ontology,
        profile:Profile ;
    dct:bibliographicCitation "Harshvardhan J. Pandit, Beatriz Esteves, Georg P. Krog, Paul Ryan, Delaram Golpayegani, Julian Flake (2025) Data Privacy Vocabulary (DPV) – Version 2.0. In: Demartini, G., et al. The Semantic Web – ISWC 2024. ISWC 2024. Lecture Notes in Computer Science, vol 15233. Springer, Cham. https://doi.org/10.1007/978-3-031-77847-6_10" ;
    dct:conformsTo <http://www.w3.org/2002/07/owl>,
        "http://www.w3.org/2000/01/rdf-schema",
        "http://www.w3.org/2004/02/skos/core" ;
    dct:contributor _:Ne8d6151e3d8047e6a947b3ec1a3830a1 ;
    dct:created "2024-05-31"@en ;
    dct:creator [ a dct:Agent,
                foaf:Person ;
            scoro:hasORCID "0000-0002-5068-3714" ;
            org:memberOf [ a foaf:Organization ;
                    foaf:name "ADAPT Centre, Dublin City University" ] ;
            foaf:homepage "https://harshp.com/" ;
            foaf:name "Harshvardhan J. Pandit" ],
        _:Ne8d6151e3d8047e6a947b3ec1a3830a1 ;
    dct:description "Extension to the Data Privacy Vocabulary (DPV) providing concepts for representing information about AI technologies"@en ;
    dct:hasVersion ai-owl: ;
    dct:identifier "https://w3id.org/dpv/ai" ;
    dct:issued "2024-05-31"@en ;
    dct:license <https://www.w3.org/copyright/document-license-2023/> ;
    dct:modified "2025-03-16"@en ;
    dct:publisher <https://www.w3.org/> ;
    dct:source <https://www.w3.org/groups/cg/dpvcg/> ;
    dct:title "AI Technology Concepts"@en ;
    bibo:doi "10.5281/zenodo.12505841" ;
    bibo:status "http://purl.org/ontology/bibo/status/published" ;
    vann:preferredNamespacePrefix "ai" ;
    vann:preferredNamespaceUri "https://w3id.org/dpv/ai#" ;
    rdfs:Label "AI"@en ;
    owl:versionIRI <https://w3id.org/dpv/2.1/ai/owl#> ;
    owl:versionInfo "2.1" ;
    profile:hasResource ai-owl:serialisation-html,
        ai-owl:serialisation-jsonld,
        ai-owl:serialisation-n3,
        ai-owl:serialisation-rdf,
        ai-owl:serialisation-ttl,
        <https://w3id.org/dpv/examples>,
        <https://w3id.org/dpv/guides>,
        <https://w3id.org/dpv/primer> ;
    profile:isProfileOf <http://www.w3.org/2002/07/owl>,
        ai-owl:,
        <https://w3id.org/dpv/tech/owl> ;
    foaf:logo <https://w3id.org/dpv/media/logo.png> ;
    schema:version "2.1" .

_:N2107ae3007164122b8f508ef58f07bab a foaf:Organization ;
    foaf:name "ADAPT Centre, Trinity College Dublin" .

_:Ne8d6151e3d8047e6a947b3ec1a3830a1 a dct:Agent,
        foaf:Person ;
    scoro:hasORCID "0000-0002-1208-186X" ;
    org:memberOf _:N2107ae3007164122b8f508ef58f07bab ;
    foaf:name "Delaram Golpayegani" .

