@prefix ai-owl: <https://w3id.org/dpv/ai/owl#> .
@prefix bibo: <http://purl.org/ontology/bibo/> .
@prefix dct: <http://purl.org/dc/terms/> .
@prefix foaf: <http://xmlns.com/foaf/0.1/> .
@prefix org: <http://www.w3.org/ns/org#> .
@prefix owl: <http://www.w3.org/2002/07/owl#> .
@prefix profile: <http://www.w3.org/ns/dx/prof/> .
@prefix rdf: <http://www.w3.org/1999/02/22-rdf-syntax-ns#> .
@prefix rdfs: <http://www.w3.org/2000/01/rdf-schema#> .
@prefix role: <http://www.w3.org/ns/dx/prof/role/> .
@prefix schema: <https://schema.org/> .
@prefix scoro: <http://purl.org/spar/scoro/> .
@prefix skos: <http://www.w3.org/2004/02/skos/core#> .
@prefix sw: <http://www.w3.org/2003/06/sw-vocab-status/ns#> .
@prefix vann: <http://purl.org/vocab/vann/> .
@prefix xsd: <http://www.w3.org/2001/XMLSchema#> .

ai-owl:AudioProcessing a rdfs:Class,
        owl:Class,
        ai-owl:Technique ;
    dct:contributor _:Ne8d6151e3d8047e6a947b3ec1a3830a1 ;
    dct:created "2024-12-01"^^xsd:date ;
    dct:source [ a schema:WebPage ;
            schema:name "AI Watch" ;
            schema:url "Defining Artificial Intelligence 2.0 [https://publications.jrc.ec.europa.eu/repository/handle/JRC126426]" ] ;
    rdfs:isDefinedBy ai-owl: ;
    rdfs:subClassOf ai-owl:Technique ;
    sw:term_status "accepted"@en ;
    skos:definition "Technique involving processing audio"@en ;
    skos:prefLabel "Audio Processing"@en .

ai-owl:BayesianEstimation a rdfs:Class,
        owl:Class,
        ai-owl:Technique ;
    dct:contributor _:Ne8d6151e3d8047e6a947b3ec1a3830a1 ;
    dct:created "2024-12-01"^^xsd:date ;
    rdfs:isDefinedBy ai-owl: ;
    rdfs:subClassOf ai-owl:StatisticalTechnique ;
    sw:term_status "accepted"@en ;
    skos:definition "Refers to Bayesian estimation approach"@en ;
    skos:prefLabel "Bayesian Estimation"@en .

ai-owl:BayesianNetwork a rdfs:Class,
        owl:Class,
        ai-owl:Technique ;
    dct:contributor _:Ne8d6151e3d8047e6a947b3ec1a3830a1 ;
    dct:created "2024-12-01"^^xsd:date ;
    dct:source " 3.3.1"@en,
        "ISO/IEC 22989"@en ;
    rdfs:isDefinedBy ai-owl: ;
    rdfs:subClassOf ai-owl:StatisticalTechnique ;
    sw:term_status "accepted"@en ;
    skos:definition "Probabilistic technique that uses Bayesian inference for probability computations using a directed acyclic graph"@en ;
    skos:prefLabel "Bayesian Network"@en .

ai-owl:BayesianOptimisation a rdfs:Class,
        owl:Class,
        ai-owl:Technique ;
    dct:contributor _:Ne8d6151e3d8047e6a947b3ec1a3830a1 ;
    dct:created "2024-12-01"^^xsd:date ;
    rdfs:isDefinedBy ai-owl: ;
    rdfs:subClassOf ai-owl:StatisticalTechnique ;
    sw:term_status "accepted"@en ;
    skos:definition "Refers to Bayesian optimisation technique"@en ;
    skos:prefLabel "Bayesian Optimisation"@en .

ai-owl:ConvolutionalNeuralNetwork a rdfs:Class,
        owl:Class,
        ai-owl:Technique ;
    dct:contributor _:Ne8d6151e3d8047e6a947b3ec1a3830a1 ;
    dct:created "2024-12-01"^^xsd:date ;
    dct:source " 3.4.2"@en,
        "ISO/IEC 22989"@en ;
    rdfs:isDefinedBy ai-owl: ;
    rdfs:subClassOf ai-owl:NeuralNetwork ;
    sw:term_status "accepted"@en ;
    skos:definition "Feed forward neural network using convolution  in at least one of its layers"@en ;
    skos:prefLabel "Convolutional Neural Network (CNN)"@en .

ai-owl:DecisionTree a rdfs:Class,
        owl:Class,
        ai-owl:Technique ;
    dct:contributor _:Ne8d6151e3d8047e6a947b3ec1a3830a1 ;
    dct:created "2024-12-01"^^xsd:date ;
    dct:source " 3.3.2"@en,
        "ISO/IEC 22989"@en ;
    rdfs:isDefinedBy ai-owl: ;
    rdfs:subClassOf ai-owl:StatisticalTechnique ;
    sw:term_status "accepted"@en ;
    skos:definition "Technique for which inference is encoded as paths from the root to a leaf node in a tree structure"@en ;
    skos:prefLabel "Decision Tree"@en .

ai-owl:DeepLearning a rdfs:Class,
        owl:Class,
        ai-owl:Technique ;
    dct:contributor _:Ne8d6151e3d8047e6a947b3ec1a3830a1 ;
    dct:created "2024-12-01"^^xsd:date ;
    dct:source " 3.4.4"@en,
        "ISO/IEC 22989:2022"@en ;
    rdfs:isDefinedBy ai-owl: ;
    rdfs:subClassOf ai-owl:MachineLearning ;
    sw:term_status "accepted"@en ;
    skos:definition "Approach to creating rich hierarchical representations through the training of neural networks with many hidden layers"@en ;
    skos:prefLabel "Deep Learning"@en .

ai-owl:FeedForwardNeuralNetwork a rdfs:Class,
        owl:Class,
        ai-owl:Technique ;
    dct:contributor _:Ne8d6151e3d8047e6a947b3ec1a3830a1 ;
    dct:created "2024-12-01"^^xsd:date ;
    dct:source " 3.4.6"@en,
        "ISO/IEC 22989"@en ;
    rdfs:isDefinedBy ai-owl: ;
    rdfs:subClassOf ai-owl:NeuralNetwork ;
    sw:term_status "accepted"@en ;
    skos:definition "Neural network where information is fed from the input layer to the output layer in one direction only"@en ;
    skos:prefLabel "Feed Forward Neural Network"@en .

ai-owl:GeneticAlgorithm a rdfs:Class,
        owl:Class,
        ai-owl:Technique ;
    dct:contributor _:Ne8d6151e3d8047e6a947b3ec1a3830a1 ;
    dct:created "2024-12-01"^^xsd:date ;
    dct:source " 3.1.15"@en,
        "ISO/IEC 22989:2022"@en ;
    rdfs:isDefinedBy ai-owl: ;
    rdfs:subClassOf ai-owl:Technique ;
    sw:term_status "accepted"@en ;
    skos:definition "Algorithm which simulates natural selection by creating and evolving a population of individuals (solutions) for optimization problems"@en ;
    skos:prefLabel "Genetic Algorithm"@en .

ai-owl:InductiveProgramming a rdfs:Class,
        owl:Class,
        ai-owl:Technique ;
    dct:contributor _:Ne8d6151e3d8047e6a947b3ec1a3830a1 ;
    dct:created "2024-12-01"^^xsd:date ;
    rdfs:isDefinedBy ai-owl: ;
    rdfs:subClassOf ai-owl:KnowledgeTechnique ;
    sw:term_status "accepted"@en ;
    skos:definition "An algorithm or program featuring recursive calls or repetition control structures"@en ;
    skos:prefLabel "Inductive Programming"@en .

ai-owl:KnowledgeRepresentation a rdfs:Class,
        owl:Class,
        ai-owl:Technique ;
    dct:contributor _:Ne8d6151e3d8047e6a947b3ec1a3830a1 ;
    dct:created "2024-12-01"^^xsd:date ;
    rdfs:isDefinedBy ai-owl: ;
    rdfs:subClassOf ai-owl:KnowledgeTechnique ;
    sw:term_status "accepted"@en ;
    skos:definition "Encoding knowledge in a formal language"@en ;
    skos:prefLabel "Knowledge Representation"@en .

ai-owl:KnowledgeTechnique a rdfs:Class,
        owl:Class,
        ai-owl:Technique ;
    dct:contributor _:Ne8d6151e3d8047e6a947b3ec1a3830a1 ;
    dct:created "2024-12-01"^^xsd:date ;
    rdfs:isDefinedBy ai-owl: ;
    rdfs:subClassOf ai-owl:Technique ;
    sw:term_status "accepted"@en ;
    skos:definition "Techniques based on the use of knowledge bases"@en ;
    skos:prefLabel "Knowledge Technique"@en .

ai-owl:LogicTechnique a rdfs:Class,
        owl:Class,
        ai-owl:Technique ;
    dct:contributor _:Ne8d6151e3d8047e6a947b3ec1a3830a1 ;
    dct:created "2024-12-01"^^xsd:date ;
    rdfs:isDefinedBy ai-owl: ;
    rdfs:subClassOf ai-owl:Technique ;
    sw:term_status "accepted"@en ;
    skos:definition "Refers to logic based techniques"@en ;
    skos:prefLabel "Logic Technique"@en .

ai-owl:LongShortTermMemory a rdfs:Class,
        owl:Class,
        ai-owl:Technique ;
    dct:contributor _:Ne8d6151e3d8047e6a947b3ec1a3830a1 ;
    dct:created "2024-12-01"^^xsd:date ;
    dct:source " 3.4.7"@en,
        "ISO/IEC 22989"@en ;
    rdfs:isDefinedBy ai-owl: ;
    rdfs:subClassOf ai-owl:NeuralNetwork ;
    sw:term_status "accepted"@en ;
    skos:definition "Type of recurrent neural network that processes sequential data with a satisfactory performance for both long and short span dependencies"@en ;
    skos:prefLabel "Long Short-Term Memory (LSTM)"@en .

ai-owl:MachineLearning a rdfs:Class,
        owl:Class,
        ai-owl:Technique ;
    dct:contributor _:Ne8d6151e3d8047e6a947b3ec1a3830a1 ;
    dct:created "2024-12-01"^^xsd:date ;
    dct:source " 3.3.5"@en,
        "ISO/IEC 22989:2022"@en ;
    rdfs:isDefinedBy ai-owl: ;
    rdfs:subClassOf ai-owl:Technique ;
    sw:term_status "accepted"@en ;
    skos:definition "Process of optimizing model parameters through computational techniques, such that the model's behaviour reflects the data or experience"@en ;
    skos:prefLabel "Machine Learning"@en .

ai-owl:NeuralNetwork a rdfs:Class,
        owl:Class,
        ai-owl:Technique ;
    dct:contributor _:Ne8d6151e3d8047e6a947b3ec1a3830a1 ;
    dct:created "2024-12-01"^^xsd:date ;
    dct:source " 3.4.8"@en,
        "ISO/IEC 22989"@en ;
    rdfs:isDefinedBy ai-owl: ;
    rdfs:subClassOf ai-owl:MachineLearning ;
    sw:term_status "accepted"@en ;
    skos:definition "Network of one or more layers of neurons connected by weighted links with adjustable weights, which takes input data and produces an output"@en ;
    skos:prefLabel "Neural Network"@en .

ai-owl:OptimisationMethod a rdfs:Class,
        owl:Class,
        ai-owl:Technique ;
    dct:contributor _:Ne8d6151e3d8047e6a947b3ec1a3830a1 ;
    dct:created "2024-12-01"^^xsd:date ;
    rdfs:isDefinedBy ai-owl: ;
    rdfs:subClassOf ai-owl:StatisticalTechnique ;
    sw:term_status "accepted"@en ;
    skos:definition "Refers to optimisation Method"@en ;
    skos:prefLabel "Optimisation Method"@en .

ai-owl:ReasoningTechnique a rdfs:Class,
        owl:Class,
        ai-owl:Technique ;
    dct:contributor _:Ne8d6151e3d8047e6a947b3ec1a3830a1 ;
    dct:created "2024-12-01"^^xsd:date ;
    rdfs:isDefinedBy ai-owl: ;
    rdfs:subClassOf ai-owl:Technique ;
    sw:term_status "accepted"@en ;
    skos:definition "Refers to reasoning techniques"@en ;
    skos:prefLabel "Reasoning Technique"@en .

ai-owl:RecurrentNeuralNetwork a rdfs:Class,
        owl:Class,
        ai-owl:Technique ;
    dct:contributor _:Ne8d6151e3d8047e6a947b3ec1a3830a1 ;
    dct:created "2024-12-01"^^xsd:date ;
    dct:source " 3.4.10"@en,
        "ISO/IEC 22989"@en ;
    rdfs:isDefinedBy ai-owl: ;
    rdfs:subClassOf ai-owl:NeuralNetwork ;
    sw:term_status "accepted"@en ;
    skos:definition "Neural network in which outputs from both the previous layer and the previous processing step are fed into the current layer"@en ;
    skos:prefLabel "Recurrent Neural Network (RNN)"@en .

ai-owl:ReinforcementLearning a rdfs:Class,
        owl:Class,
        ai-owl:Technique ;
    dct:contributor _:Ne8d6151e3d8047e6a947b3ec1a3830a1 ;
    dct:created "2024-12-01"^^xsd:date ;
    dct:source " 3.3.9"@en,
        "ISO/IEC 22989:2022"@en ;
    rdfs:isDefinedBy ai-owl: ;
    rdfs:subClassOf ai-owl:MachineLearning ;
    sw:term_status "accepted"@en ;
    skos:definition "Learning of an optimal sequence of actions to maximize a reward through interaction with an environment"@en ;
    skos:prefLabel "Reinforcement Learning"@en .

ai-owl:SearchMethod a rdfs:Class,
        owl:Class,
        ai-owl:Technique ;
    dct:contributor _:Ne8d6151e3d8047e6a947b3ec1a3830a1 ;
    dct:created "2024-12-01"^^xsd:date ;
    rdfs:isDefinedBy ai-owl: ;
    rdfs:subClassOf ai-owl:StatisticalTechnique ;
    sw:term_status "accepted"@en ;
    skos:definition "Refers to statistical-based search Methods"@en ;
    skos:prefLabel "Search Method"@en .

ai-owl:SemiSupervisedLearning a rdfs:Class,
        owl:Class,
        ai-owl:Technique ;
    dct:contributor _:Ne8d6151e3d8047e6a947b3ec1a3830a1 ;
    dct:created "2024-12-01"^^xsd:date ;
    dct:source " 3.3.11"@en,
        "ISO/IEC 22989:2022"@en ;
    rdfs:isDefinedBy ai-owl: ;
    rdfs:subClassOf ai-owl:MachineLearning ;
    sw:term_status "accepted"@en ;
    skos:definition "Machine learning that makes use of both labelled and unlabelled data during training"@en ;
    skos:prefLabel "Semi Supervised Learning"@en .

ai-owl:StatisticalTechnique a rdfs:Class,
        owl:Class,
        ai-owl:Technique ;
    dct:contributor _:Ne8d6151e3d8047e6a947b3ec1a3830a1 ;
    dct:created "2024-12-01"^^xsd:date ;
    rdfs:isDefinedBy ai-owl: ;
    rdfs:subClassOf ai-owl:Technique ;
    sw:term_status "accepted"@en ;
    skos:definition "Refers to techniques that are based on statistics"@en ;
    skos:prefLabel "Statistical Technique"@en .

ai-owl:SupervisedLearning a rdfs:Class,
        owl:Class,
        ai-owl:Technique ;
    dct:contributor _:Ne8d6151e3d8047e6a947b3ec1a3830a1 ;
    dct:created "2024-12-01"^^xsd:date ;
    dct:source " 3.3.11"@en,
        "ISO/IEC 22989:2022"@en ;
    rdfs:isDefinedBy ai-owl: ;
    rdfs:subClassOf ai-owl:MachineLearning ;
    sw:term_status "accepted"@en ;
    skos:definition "Machine learning that makes only use of labelled data during training"@en ;
    skos:prefLabel "Supervised Learning"@en .

ai-owl:SupportVectorMachine a rdfs:Class,
        owl:Class,
        ai-owl:Technique ;
    dct:contributor _:Ne8d6151e3d8047e6a947b3ec1a3830a1 ;
    dct:created "2024-12-01"^^xsd:date ;
    dct:source " 3.3.13"@en,
        "ISO/IEC 22989"@en ;
    rdfs:isDefinedBy ai-owl: ;
    rdfs:subClassOf ai-owl:MachineLearning ;
    sw:term_status "accepted"@en ;
    skos:definition "A machine learning algorithm that finds decision boundaries with maximal margins"@en ;
    skos:prefLabel "Support Vector Machine"@en .

ai-owl:SymbolicReasoning a rdfs:Class,
        owl:Class,
        ai-owl:Technique ;
    dct:contributor _:Ne8d6151e3d8047e6a947b3ec1a3830a1 ;
    dct:created "2024-12-01"^^xsd:date ;
    rdfs:isDefinedBy ai-owl: ;
    rdfs:subClassOf ai-owl:KnowledgeTechnique ;
    sw:term_status "accepted"@en ;
    skos:definition "Reasoning based on the knowledge encoded in a formal language"@en ;
    skos:prefLabel "Symbolic Reasoning"@en .

ai-owl:UnsupervisedLearning a rdfs:Class,
        owl:Class,
        ai-owl:Technique ;
    dct:contributor _:Ne8d6151e3d8047e6a947b3ec1a3830a1 ;
    dct:created "2024-12-01"^^xsd:date ;
    dct:source " 3.3.17"@en,
        "ISO/IEC 22989:2022"@en ;
    rdfs:isDefinedBy ai-owl: ;
    rdfs:subClassOf ai-owl:MachineLearning ;
    sw:term_status "accepted"@en ;
    skos:definition "Machine learning that makes only use of unlabelled data during training"@en ;
    skos:prefLabel "Unsupervised Learning"@en .

ai-owl:serialisation-html a profile:ResourceDescriptor ;
    dct:conformsTo <https://www.w3.org/TR/html/> ;
    dct:format <https://www.iana.org/assignments/media-types/text/html> ;
    dct:title "AI Technology Concepts - HTML serialiation" ;
    profile:hasArtifact <https://w3id.org/dpv/ai/ai-owl.html> ;
    profile:hasRole role:specification .

ai-owl:serialisation-jsonld a profile:ResourceDescriptor ;
    dct:conformsTo <https://www.w3.org/TR/json-ld11/> ;
    dct:format <https://www.iana.org/assignments/media-types/application/ld+json> ;
    dct:title "AI Technology Concepts - JSON-LD serialiation" ;
    profile:hasArtifact <https://w3id.org/dpv/ai/ai-owl.jsonld> ;
    profile:hasRole role:vocabulary .

ai-owl:serialisation-n3 a profile:ResourceDescriptor ;
    dct:conformsTo <https://www.w3.org/TeamSubmission/n3/> ;
    dct:format <https://www.iana.org/assignments/media-types/text/n3> ;
    dct:title "AI Technology Concepts - N3 serialiation" ;
    profile:hasArtifact <https://w3id.org/dpv/ai/ai-owl.n3> ;
    profile:hasRole role:vocabulary .

ai-owl:serialisation-rdf a profile:ResourceDescriptor ;
    dct:conformsTo rdf: ;
    dct:format <https://www.iana.org/assignments/media-types/application/rdf+xml> ;
    dct:title "AI Technology Concepts - RDF/XML serialiation" ;
    profile:hasArtifact <https://w3id.org/dpv/ai/ai-owl.rdf> ;
    profile:hasRole role:vocabulary .

ai-owl:serialisation-ttl a profile:ResourceDescriptor ;
    dct:conformsTo <https://www.w3.org/TR/turtle/> ;
    dct:format <https://www.iana.org/assignments/media-types/text/turtle> ;
    dct:title "AI Technology Concepts - Turtle serialiation" ;
    profile:hasArtifact <https://w3id.org/dpv/ai/ai-owl.ttl> ;
    profile:hasRole role:vocabulary .

<https://w3id.org/dpv/examples> a profile:ResourceDescriptor ;
    dct:conformsTo <https://www.w3.org/TR/html/> ;
    dct:format <https://www.iana.org/assignments/media-types/text/html> ;
    dct:title "Examples for Data Privacy Vocabulary" ;
    profile:hasArtifact <https://w3id.org/dpv/examples> ;
    profile:hasRole role:guidance .

<https://w3id.org/dpv/guides> a profile:ResourceDescriptor ;
    dct:conformsTo <https://www.w3.org/TR/html/> ;
    dct:format <https://www.iana.org/assignments/media-types/text/html> ;
    dct:title "Guides for Data Privacy Vocabulary" ;
    profile:hasArtifact <https://w3id.org/dpv/guides> ;
    profile:hasRole role:guidance .

<https://w3id.org/dpv/primer> a profile:ResourceDescriptor ;
    dct:conformsTo <https://www.w3.org/TR/html/> ;
    dct:format <https://www.iana.org/assignments/media-types/text/html> ;
    dct:title "Primer for Data Privacy Vocabulary" ;
    profile:hasArtifact <https://w3id.org/dpv/primer> ;
    profile:hasRole role:guidance .

ai-owl: a owl:Ontology,
        profile:Profile ;
    dct:bibliographicCitation "Harshvardhan J. Pandit, Beatriz Esteves, Georg P. Krog, Paul Ryan, Delaram Golpayegani, Julian Flake (2025) Data Privacy Vocabulary (DPV) – Version 2.0. In: Demartini, G., et al. The Semantic Web – ISWC 2024. ISWC 2024. Lecture Notes in Computer Science, vol 15233. Springer, Cham. https://doi.org/10.1007/978-3-031-77847-6_10" ;
    dct:conformsTo <http://www.w3.org/2002/07/owl>,
        "http://www.w3.org/2000/01/rdf-schema",
        "http://www.w3.org/2004/02/skos/core" ;
    dct:contributor _:Ne8d6151e3d8047e6a947b3ec1a3830a1 ;
    dct:created "2024-05-31"@en ;
    dct:creator [ a dct:Agent,
                foaf:Person ;
            scoro:hasORCID "0000-0002-5068-3714" ;
            org:memberOf [ a foaf:Organization ;
                    foaf:name "ADAPT Centre, Dublin City University" ] ;
            foaf:homepage "https://harshp.com/" ;
            foaf:name "Harshvardhan J. Pandit" ],
        _:Ne8d6151e3d8047e6a947b3ec1a3830a1 ;
    dct:description "Extension to the Data Privacy Vocabulary (DPV) providing concepts for representing information about AI technologies"@en ;
    dct:hasVersion ai-owl: ;
    dct:identifier "https://w3id.org/dpv/ai" ;
    dct:issued "2024-05-31"@en ;
    dct:license <https://www.w3.org/copyright/document-license-2023/> ;
    dct:modified "2025-03-16"@en ;
    dct:publisher <https://www.w3.org/> ;
    dct:source <https://www.w3.org/groups/cg/dpvcg/> ;
    dct:title "AI Technology Concepts"@en ;
    bibo:doi "10.5281/zenodo.12505841" ;
    bibo:status "http://purl.org/ontology/bibo/status/published" ;
    vann:preferredNamespacePrefix "ai" ;
    vann:preferredNamespaceUri "https://w3id.org/dpv/ai#" ;
    rdfs:Label "AI"@en ;
    owl:versionIRI <https://w3id.org/dpv/2.1/ai/owl#> ;
    owl:versionInfo "2.1" ;
    profile:hasResource ai-owl:serialisation-html,
        ai-owl:serialisation-jsonld,
        ai-owl:serialisation-n3,
        ai-owl:serialisation-rdf,
        ai-owl:serialisation-ttl,
        <https://w3id.org/dpv/examples>,
        <https://w3id.org/dpv/guides>,
        <https://w3id.org/dpv/primer> ;
    profile:isProfileOf <http://www.w3.org/2002/07/owl>,
        ai-owl:,
        <https://w3id.org/dpv/tech/owl> ;
    foaf:logo <https://w3id.org/dpv/media/logo.png> ;
    schema:version "2.1" .

_:N2107ae3007164122b8f508ef58f07bab a foaf:Organization ;
    foaf:name "ADAPT Centre, Trinity College Dublin" .

_:Ne8d6151e3d8047e6a947b3ec1a3830a1 a dct:Agent,
        foaf:Person ;
    scoro:hasORCID "0000-0002-1208-186X" ;
    org:memberOf _:N2107ae3007164122b8f508ef58f07bab ;
    foaf:name "Delaram Golpayegani" .

