@prefix bibo: <http://purl.org/ontology/bibo/> .
@prefix dct: <http://purl.org/dc/terms/> .
@prefix dpv: <https://w3id.org/dpv#> .
@prefix eu-rights: <https://w3id.org/dpv/rights/eu#> .
@prefix foaf: <http://xmlns.com/foaf/0.1/> .
@prefix org: <http://www.w3.org/ns/org#> .
@prefix owl: <http://www.w3.org/2002/07/owl#> .
@prefix profile: <http://www.w3.org/ns/dx/prof/> .
@prefix rdf: <http://www.w3.org/1999/02/22-rdf-syntax-ns#> .
@prefix rdfs: <http://www.w3.org/2000/01/rdf-schema#> .
@prefix risk: <https://w3id.org/dpv/risk#> .
@prefix role: <http://www.w3.org/ns/dx/prof/role/> .
@prefix schema: <https://schema.org/> .
@prefix scoro: <http://purl.org/spar/scoro/> .
@prefix skos: <http://www.w3.org/2004/02/skos/core#> .
@prefix sw: <http://www.w3.org/2003/06/sw-vocab-status/ns#> .
@prefix vann: <http://purl.org/vocab/vann/> .
@prefix xsd: <http://www.w3.org/2001/XMLSchema#> .

eu-rights:A1-HumanDignityImpact a rdfs:Class,
        skos:Concept,
        dpv:RiskConcept,
        risk:PotentialConsequence,
        risk:PotentialImpact,
        risk:PotentialRisk ;
    dct:contributor _:N0a43dd9ea5e94fe695d8b7df8802cfdd ;
    dct:created "2022-06-24"^^xsd:date ;
    dct:source [ a schema:WebPage ;
            schema:name "Charter of Fundamental Rights of the European Union" ;
            schema:url "http://data.europa.eu/eli/treaty/char_2012/oj" ] ;
    rdfs:isDefinedBy eu-rights: ;
    sw:term_status "accepted"@en ;
    skos:broader eu-rights:T1-DignityImpact ;
    skos:definition "Something that acts as or is considered as an impact on A1 Human Dignity"@en ;
    skos:inScheme eu-rights:impacts-classes ;
    skos:prefLabel "Impact on A1 Human Dignity"@en .

eu-rights:A10-FreedomOfThoughtConscienceReligionImpact a rdfs:Class,
        skos:Concept,
        dpv:RiskConcept,
        risk:PotentialConsequence,
        risk:PotentialImpact,
        risk:PotentialRisk ;
    dct:contributor _:N0a43dd9ea5e94fe695d8b7df8802cfdd ;
    dct:created "2022-07-04"^^xsd:date ;
    dct:source [ a schema:WebPage ;
            schema:name "Charter of Fundamental Rights of the European Union" ;
            schema:url "http://data.europa.eu/eli/treaty/char_2012/oj" ] ;
    rdfs:isDefinedBy eu-rights: ;
    sw:term_status "accepted"@en ;
    skos:broader eu-rights:T2-FreedomsImpact ;
    skos:definition "Something that acts as or is considered as an impact on A10 Freedom Of Thought Conscience Religion"@en ;
    skos:inScheme eu-rights:impacts-classes ;
    skos:prefLabel "Impact on A10 Freedom Of Thought Conscience Religion"@en .

eu-rights:A11-FreedomOfExpressionInformationImpact a rdfs:Class,
        skos:Concept,
        dpv:RiskConcept,
        risk:PotentialConsequence,
        risk:PotentialImpact,
        risk:PotentialRisk ;
    dct:contributor _:N0a43dd9ea5e94fe695d8b7df8802cfdd ;
    dct:created "2022-07-05"^^xsd:date ;
    dct:source [ a schema:WebPage ;
            schema:name "Charter of Fundamental Rights of the European Union" ;
            schema:url "http://data.europa.eu/eli/treaty/char_2012/oj" ] ;
    rdfs:isDefinedBy eu-rights: ;
    sw:term_status "accepted"@en ;
    skos:broader eu-rights:T2-FreedomsImpact ;
    skos:definition "Something that acts as or is considered as an impact on A11 Freedom Of Expression Information"@en ;
    skos:inScheme eu-rights:impacts-classes ;
    skos:prefLabel "Impact on A11 Freedom Of Expression Information"@en .

eu-rights:A12-FreedomOfAssemblyAssociationImpact a rdfs:Class,
        skos:Concept,
        dpv:RiskConcept,
        risk:PotentialConsequence,
        risk:PotentialImpact,
        risk:PotentialRisk ;
    dct:contributor _:N0a43dd9ea5e94fe695d8b7df8802cfdd ;
    dct:created "2022-07-06"^^xsd:date ;
    dct:source [ a schema:WebPage ;
            schema:name "Charter of Fundamental Rights of the European Union" ;
            schema:url "http://data.europa.eu/eli/treaty/char_2012/oj" ] ;
    rdfs:isDefinedBy eu-rights: ;
    sw:term_status "accepted"@en ;
    skos:broader eu-rights:T2-FreedomsImpact ;
    skos:definition "Something that acts as or is considered as an impact on A12 Freedom Of Assembly Association"@en ;
    skos:inScheme eu-rights:impacts-classes ;
    skos:prefLabel "Impact on A12 Freedom Of Assembly Association"@en .

eu-rights:A13-FreedomOfArtsSciencesImpact a rdfs:Class,
        skos:Concept,
        dpv:RiskConcept,
        risk:PotentialConsequence,
        risk:PotentialImpact,
        risk:PotentialRisk ;
    dct:contributor _:N0a43dd9ea5e94fe695d8b7df8802cfdd ;
    dct:created "2022-07-07"^^xsd:date ;
    dct:source [ a schema:WebPage ;
            schema:name "Charter of Fundamental Rights of the European Union" ;
            schema:url "http://data.europa.eu/eli/treaty/char_2012/oj" ] ;
    rdfs:isDefinedBy eu-rights: ;
    sw:term_status "accepted"@en ;
    skos:broader eu-rights:T2-FreedomsImpact ;
    skos:definition "Something that acts as or is considered as an impact on A13 Freedom Of Arts Sciences"@en ;
    skos:inScheme eu-rights:impacts-classes ;
    skos:prefLabel "Impact on A13 Freedom Of Arts Sciences"@en .

eu-rights:A14-RightToEducationImpact a rdfs:Class,
        skos:Concept,
        dpv:RiskConcept,
        risk:PotentialConsequence,
        risk:PotentialImpact,
        risk:PotentialRisk ;
    dct:contributor _:N0a43dd9ea5e94fe695d8b7df8802cfdd ;
    dct:created "2022-07-08"^^xsd:date ;
    dct:source [ a schema:WebPage ;
            schema:name "Charter of Fundamental Rights of the European Union" ;
            schema:url "http://data.europa.eu/eli/treaty/char_2012/oj" ] ;
    rdfs:isDefinedBy eu-rights: ;
    sw:term_status "accepted"@en ;
    skos:broader eu-rights:T2-FreedomsImpact ;
    skos:definition "Something that acts as or is considered as an impact on A14 Right To Education"@en ;
    skos:inScheme eu-rights:impacts-classes ;
    skos:prefLabel "Impact on A14 Right To Education"@en .

eu-rights:A15-FreedomToChooseOccupationEngageWorkImpact a rdfs:Class,
        skos:Concept,
        dpv:RiskConcept,
        risk:PotentialConsequence,
        risk:PotentialImpact,
        risk:PotentialRisk ;
    dct:contributor _:N0a43dd9ea5e94fe695d8b7df8802cfdd ;
    dct:created "2022-07-09"^^xsd:date ;
    dct:source [ a schema:WebPage ;
            schema:name "Charter of Fundamental Rights of the European Union" ;
            schema:url "http://data.europa.eu/eli/treaty/char_2012/oj" ] ;
    rdfs:isDefinedBy eu-rights: ;
    sw:term_status "accepted"@en ;
    skos:broader eu-rights:T2-FreedomsImpact ;
    skos:definition "Something that acts as or is considered as an impact on A15 Freedom To Choose Occupation Engage Work"@en ;
    skos:inScheme eu-rights:impacts-classes ;
    skos:prefLabel "Impact on A15 Freedom To Choose Occupation Engage Work"@en .

eu-rights:A16-FreedomToConductBusinessImpact a rdfs:Class,
        skos:Concept,
        dpv:RiskConcept,
        risk:PotentialConsequence,
        risk:PotentialImpact,
        risk:PotentialRisk ;
    dct:contributor _:N0a43dd9ea5e94fe695d8b7df8802cfdd ;
    dct:created "2022-07-10"^^xsd:date ;
    dct:source [ a schema:WebPage ;
            schema:name "Charter of Fundamental Rights of the European Union" ;
            schema:url "http://data.europa.eu/eli/treaty/char_2012/oj" ] ;
    rdfs:isDefinedBy eu-rights: ;
    sw:term_status "accepted"@en ;
    skos:broader eu-rights:T2-FreedomsImpact ;
    skos:definition "Something that acts as or is considered as an impact on A16 Freedom To Conduct Business"@en ;
    skos:inScheme eu-rights:impacts-classes ;
    skos:prefLabel "Impact on A16 Freedom To Conduct Business"@en .

eu-rights:A17-RightToPropertyImpact a rdfs:Class,
        skos:Concept,
        dpv:RiskConcept,
        risk:PotentialConsequence,
        risk:PotentialImpact,
        risk:PotentialRisk ;
    dct:contributor _:N0a43dd9ea5e94fe695d8b7df8802cfdd ;
    dct:created "2022-07-11"^^xsd:date ;
    dct:source [ a schema:WebPage ;
            schema:name "Charter of Fundamental Rights of the European Union" ;
            schema:url "http://data.europa.eu/eli/treaty/char_2012/oj" ] ;
    rdfs:isDefinedBy eu-rights: ;
    sw:term_status "accepted"@en ;
    skos:broader eu-rights:T2-FreedomsImpact ;
    skos:definition "Something that acts as or is considered as an impact on A17 Right To Property"@en ;
    skos:inScheme eu-rights:impacts-classes ;
    skos:prefLabel "Impact on A17 Right To Property"@en .

eu-rights:A18-RightToAsylumImpact a rdfs:Class,
        skos:Concept,
        dpv:RiskConcept,
        risk:PotentialConsequence,
        risk:PotentialImpact,
        risk:PotentialRisk ;
    dct:contributor _:N0a43dd9ea5e94fe695d8b7df8802cfdd ;
    dct:created "2022-07-12"^^xsd:date ;
    dct:source [ a schema:WebPage ;
            schema:name "Charter of Fundamental Rights of the European Union" ;
            schema:url "http://data.europa.eu/eli/treaty/char_2012/oj" ] ;
    rdfs:isDefinedBy eu-rights: ;
    sw:term_status "accepted"@en ;
    skos:broader eu-rights:T2-FreedomsImpact ;
    skos:definition "Something that acts as or is considered as an impact on A18 Right To Asylum"@en ;
    skos:inScheme eu-rights:impacts-classes ;
    skos:prefLabel "Impact on A18 Right To Asylum"@en .

eu-rights:A19-ProtectionRemovalExpulsionExtraditionImpact a rdfs:Class,
        skos:Concept,
        dpv:RiskConcept,
        risk:PotentialConsequence,
        risk:PotentialImpact,
        risk:PotentialRisk ;
    dct:contributor _:N0a43dd9ea5e94fe695d8b7df8802cfdd ;
    dct:created "2022-07-13"^^xsd:date ;
    dct:source [ a schema:WebPage ;
            schema:name "Charter of Fundamental Rights of the European Union" ;
            schema:url "http://data.europa.eu/eli/treaty/char_2012/oj" ] ;
    rdfs:isDefinedBy eu-rights: ;
    sw:term_status "accepted"@en ;
    skos:broader eu-rights:T2-FreedomsImpact ;
    skos:definition "Something that acts as or is considered as an impact on A19 Protection Removal Expulsion Extradition"@en ;
    skos:inScheme eu-rights:impacts-classes ;
    skos:prefLabel "Impact on A19 Protection Removal Expulsion Extradition"@en .

eu-rights:A2-RightToLifeImpact a rdfs:Class,
        skos:Concept,
        dpv:RiskConcept,
        risk:PotentialConsequence,
        risk:PotentialImpact,
        risk:PotentialRisk ;
    dct:contributor _:N0a43dd9ea5e94fe695d8b7df8802cfdd ;
    dct:created "2022-06-25"^^xsd:date ;
    dct:source [ a schema:WebPage ;
            schema:name "Charter of Fundamental Rights of the European Union" ;
            schema:url "http://data.europa.eu/eli/treaty/char_2012/oj" ] ;
    rdfs:isDefinedBy eu-rights: ;
    sw:term_status "accepted"@en ;
    skos:broader eu-rights:T1-DignityImpact ;
    skos:definition "Something that acts as or is considered as an impact on A2 Right To Life"@en ;
    skos:inScheme eu-rights:impacts-classes ;
    skos:prefLabel "Impact on A2 Right To Life"@en .

eu-rights:A20-EqualityBeforeLawImpact a rdfs:Class,
        skos:Concept,
        dpv:RiskConcept,
        risk:PotentialConsequence,
        risk:PotentialImpact,
        risk:PotentialRisk ;
    dct:contributor _:N0a43dd9ea5e94fe695d8b7df8802cfdd ;
    dct:created "2022-07-15"^^xsd:date ;
    dct:source [ a schema:WebPage ;
            schema:name "Charter of Fundamental Rights of the European Union" ;
            schema:url "http://data.europa.eu/eli/treaty/char_2012/oj" ] ;
    rdfs:isDefinedBy eu-rights: ;
    sw:term_status "accepted"@en ;
    skos:broader eu-rights:T3-EqualityImpact ;
    skos:definition "Something that acts as or is considered as an impact on A20 Equality Before Law"@en ;
    skos:inScheme eu-rights:impacts-classes ;
    skos:prefLabel "Impact on A20 Equality Before Law"@en .

eu-rights:A21-NonDiscriminationImpact a rdfs:Class,
        skos:Concept,
        dpv:RiskConcept,
        risk:PotentialConsequence,
        risk:PotentialImpact,
        risk:PotentialRisk ;
    dct:contributor _:N0a43dd9ea5e94fe695d8b7df8802cfdd ;
    dct:created "2022-07-16"^^xsd:date ;
    dct:source [ a schema:WebPage ;
            schema:name "Charter of Fundamental Rights of the European Union" ;
            schema:url "http://data.europa.eu/eli/treaty/char_2012/oj" ] ;
    rdfs:isDefinedBy eu-rights: ;
    sw:term_status "accepted"@en ;
    skos:broader eu-rights:T3-EqualityImpact ;
    skos:definition "Something that acts as or is considered as an impact on A21 Non Discrimination"@en ;
    skos:inScheme eu-rights:impacts-classes ;
    skos:prefLabel "Impact on A21 Non Discrimination"@en .

eu-rights:A22-CulturalReligiousLinguisticDiversityImpact a rdfs:Class,
        skos:Concept,
        dpv:RiskConcept,
        risk:PotentialConsequence,
        risk:PotentialImpact,
        risk:PotentialRisk ;
    dct:contributor _:N0a43dd9ea5e94fe695d8b7df8802cfdd ;
    dct:created "2022-07-17"^^xsd:date ;
    dct:source [ a schema:WebPage ;
            schema:name "Charter of Fundamental Rights of the European Union" ;
            schema:url "http://data.europa.eu/eli/treaty/char_2012/oj" ] ;
    rdfs:isDefinedBy eu-rights: ;
    sw:term_status "accepted"@en ;
    skos:broader eu-rights:T3-EqualityImpact ;
    skos:definition "Something that acts as or is considered as an impact on A22 Cultural Religious Linguistic Diversity"@en ;
    skos:inScheme eu-rights:impacts-classes ;
    skos:prefLabel "Impact on A22 Cultural Religious Linguistic Diversity"@en .

eu-rights:A23-EqualityBetweenWomenMenImpact a rdfs:Class,
        skos:Concept,
        dpv:RiskConcept,
        risk:PotentialConsequence,
        risk:PotentialImpact,
        risk:PotentialRisk ;
    dct:contributor _:N0a43dd9ea5e94fe695d8b7df8802cfdd ;
    dct:created "2022-07-18"^^xsd:date ;
    dct:source [ a schema:WebPage ;
            schema:name "Charter of Fundamental Rights of the European Union" ;
            schema:url "http://data.europa.eu/eli/treaty/char_2012/oj" ] ;
    rdfs:isDefinedBy eu-rights: ;
    sw:term_status "accepted"@en ;
    skos:broader eu-rights:T3-EqualityImpact ;
    skos:definition "Something that acts as or is considered as an impact on A23 Equality Between Women Men"@en ;
    skos:inScheme eu-rights:impacts-classes ;
    skos:prefLabel "Impact on A23 Equality Between Women Men"@en .

eu-rights:A24-RightsOfChildImpact a rdfs:Class,
        skos:Concept,
        dpv:RiskConcept,
        risk:PotentialConsequence,
        risk:PotentialImpact,
        risk:PotentialRisk ;
    dct:contributor _:N0a43dd9ea5e94fe695d8b7df8802cfdd ;
    dct:created "2022-07-19"^^xsd:date ;
    dct:source [ a schema:WebPage ;
            schema:name "Charter of Fundamental Rights of the European Union" ;
            schema:url "http://data.europa.eu/eli/treaty/char_2012/oj" ] ;
    rdfs:isDefinedBy eu-rights: ;
    sw:term_status "accepted"@en ;
    skos:broader eu-rights:T3-EqualityImpact ;
    skos:definition "Something that acts as or is considered as an impact on A24 Rights Of Child"@en ;
    skos:inScheme eu-rights:impacts-classes ;
    skos:prefLabel "Impact on A24 Rights Of Child"@en .

eu-rights:A25-RightsOfElderlyImpact a rdfs:Class,
        skos:Concept,
        dpv:RiskConcept,
        risk:PotentialConsequence,
        risk:PotentialImpact,
        risk:PotentialRisk ;
    dct:contributor _:N0a43dd9ea5e94fe695d8b7df8802cfdd ;
    dct:created "2022-07-20"^^xsd:date ;
    dct:source [ a schema:WebPage ;
            schema:name "Charter of Fundamental Rights of the European Union" ;
            schema:url "http://data.europa.eu/eli/treaty/char_2012/oj" ] ;
    rdfs:isDefinedBy eu-rights: ;
    sw:term_status "accepted"@en ;
    skos:broader eu-rights:T3-EqualityImpact ;
    skos:definition "Something that acts as or is considered as an impact on A25 Rights Of Elderly"@en ;
    skos:inScheme eu-rights:impacts-classes ;
    skos:prefLabel "Impact on A25 Rights Of Elderly"@en .

eu-rights:A26-IntegrationOfPersonsWithDisabilitiesImpact a rdfs:Class,
        skos:Concept,
        dpv:RiskConcept,
        risk:PotentialConsequence,
        risk:PotentialImpact,
        risk:PotentialRisk ;
    dct:contributor _:N0a43dd9ea5e94fe695d8b7df8802cfdd ;
    dct:created "2022-07-21"^^xsd:date ;
    dct:source [ a schema:WebPage ;
            schema:name "Charter of Fundamental Rights of the European Union" ;
            schema:url "http://data.europa.eu/eli/treaty/char_2012/oj" ] ;
    rdfs:isDefinedBy eu-rights: ;
    sw:term_status "accepted"@en ;
    skos:broader eu-rights:T3-EqualityImpact ;
    skos:definition "Something that acts as or is considered as an impact on A26 Integration Of Persons With Disabilities"@en ;
    skos:inScheme eu-rights:impacts-classes ;
    skos:prefLabel "Impact on A26 Integration Of Persons With Disabilities"@en .

eu-rights:A27-WorkersRightToInformationConsultationImpact a rdfs:Class,
        skos:Concept,
        dpv:RiskConcept,
        risk:PotentialConsequence,
        risk:PotentialImpact,
        risk:PotentialRisk ;
    dct:contributor _:N0a43dd9ea5e94fe695d8b7df8802cfdd ;
    dct:created "2022-07-23"^^xsd:date ;
    dct:source [ a schema:WebPage ;
            schema:name "Charter of Fundamental Rights of the European Union" ;
            schema:url "http://data.europa.eu/eli/treaty/char_2012/oj" ] ;
    rdfs:isDefinedBy eu-rights: ;
    sw:term_status "accepted"@en ;
    skos:broader eu-rights:T4-SolidarityImpact ;
    skos:definition "Something that acts as or is considered as an impact on A27 Workers Right To Information Consultation"@en ;
    skos:inScheme eu-rights:impacts-classes ;
    skos:prefLabel "Impact on A27 Workers Right To Information Consultation"@en .

eu-rights:A28-RightOfCollectiveBargainingActionImpact a rdfs:Class,
        skos:Concept,
        dpv:RiskConcept,
        risk:PotentialConsequence,
        risk:PotentialImpact,
        risk:PotentialRisk ;
    dct:contributor _:N0a43dd9ea5e94fe695d8b7df8802cfdd ;
    dct:created "2022-07-24"^^xsd:date ;
    dct:source [ a schema:WebPage ;
            schema:name "Charter of Fundamental Rights of the European Union" ;
            schema:url "http://data.europa.eu/eli/treaty/char_2012/oj" ] ;
    rdfs:isDefinedBy eu-rights: ;
    sw:term_status "accepted"@en ;
    skos:broader eu-rights:T4-SolidarityImpact ;
    skos:definition "Something that acts as or is considered as an impact on A28 Right Of Collective Bargaining Action"@en ;
    skos:inScheme eu-rights:impacts-classes ;
    skos:prefLabel "Impact on A28 Right Of Collective Bargaining Action"@en .

eu-rights:A29-RightOfAccessToPlacementServicesImpact a rdfs:Class,
        skos:Concept,
        dpv:RiskConcept,
        risk:PotentialConsequence,
        risk:PotentialImpact,
        risk:PotentialRisk ;
    dct:contributor _:N0a43dd9ea5e94fe695d8b7df8802cfdd ;
    dct:created "2022-07-25"^^xsd:date ;
    dct:source [ a schema:WebPage ;
            schema:name "Charter of Fundamental Rights of the European Union" ;
            schema:url "http://data.europa.eu/eli/treaty/char_2012/oj" ] ;
    rdfs:isDefinedBy eu-rights: ;
    sw:term_status "accepted"@en ;
    skos:broader eu-rights:T4-SolidarityImpact ;
    skos:definition "Something that acts as or is considered as an impact on A29 Right Of Access To Placement Services"@en ;
    skos:inScheme eu-rights:impacts-classes ;
    skos:prefLabel "Impact on A29 Right Of Access To Placement Services"@en .

eu-rights:A3-RightToIntegrityOfPersonImpact a rdfs:Class,
        skos:Concept,
        dpv:RiskConcept,
        risk:PotentialConsequence,
        risk:PotentialImpact,
        risk:PotentialRisk ;
    dct:contributor _:N0a43dd9ea5e94fe695d8b7df8802cfdd ;
    dct:created "2022-06-26"^^xsd:date ;
    dct:source [ a schema:WebPage ;
            schema:name "Charter of Fundamental Rights of the European Union" ;
            schema:url "http://data.europa.eu/eli/treaty/char_2012/oj" ] ;
    rdfs:isDefinedBy eu-rights: ;
    sw:term_status "accepted"@en ;
    skos:broader eu-rights:T1-DignityImpact ;
    skos:definition "Something that acts as or is considered as an impact on A3 Right To Integrity Of Person"@en ;
    skos:inScheme eu-rights:impacts-classes ;
    skos:prefLabel "Impact on A3 Right To Integrity Of Person"@en .

eu-rights:A30-ProtectionUnjustifiedDismissalImpact a rdfs:Class,
        skos:Concept,
        dpv:RiskConcept,
        risk:PotentialConsequence,
        risk:PotentialImpact,
        risk:PotentialRisk ;
    dct:contributor _:N0a43dd9ea5e94fe695d8b7df8802cfdd ;
    dct:created "2022-07-26"^^xsd:date ;
    dct:source [ a schema:WebPage ;
            schema:name "Charter of Fundamental Rights of the European Union" ;
            schema:url "http://data.europa.eu/eli/treaty/char_2012/oj" ] ;
    rdfs:isDefinedBy eu-rights: ;
    sw:term_status "accepted"@en ;
    skos:broader eu-rights:T4-SolidarityImpact ;
    skos:definition "Something that acts as or is considered as an impact on A30 Protection Unjustified Dismissal"@en ;
    skos:inScheme eu-rights:impacts-classes ;
    skos:prefLabel "Impact on A30 Protection Unjustified Dismissal"@en .

eu-rights:A31-FairJustWorkingConditionsImpact a rdfs:Class,
        skos:Concept,
        dpv:RiskConcept,
        risk:PotentialConsequence,
        risk:PotentialImpact,
        risk:PotentialRisk ;
    dct:contributor _:N0a43dd9ea5e94fe695d8b7df8802cfdd ;
    dct:created "2022-07-27"^^xsd:date ;
    dct:source [ a schema:WebPage ;
            schema:name "Charter of Fundamental Rights of the European Union" ;
            schema:url "http://data.europa.eu/eli/treaty/char_2012/oj" ] ;
    rdfs:isDefinedBy eu-rights: ;
    sw:term_status "accepted"@en ;
    skos:broader eu-rights:T4-SolidarityImpact ;
    skos:definition "Something that acts as or is considered as an impact on A31 Fair Just Working Conditions"@en ;
    skos:inScheme eu-rights:impacts-classes ;
    skos:prefLabel "Impact on A31 Fair Just Working Conditions"@en .

eu-rights:A32-ProhibitionOfChildLabourProtectionofYoungAtWorkImpact a rdfs:Class,
        skos:Concept,
        dpv:RiskConcept,
        risk:PotentialConsequence,
        risk:PotentialImpact,
        risk:PotentialRisk ;
    dct:contributor _:N0a43dd9ea5e94fe695d8b7df8802cfdd ;
    dct:created "2022-07-28"^^xsd:date ;
    dct:source [ a schema:WebPage ;
            schema:name "Charter of Fundamental Rights of the European Union" ;
            schema:url "http://data.europa.eu/eli/treaty/char_2012/oj" ] ;
    rdfs:isDefinedBy eu-rights: ;
    sw:term_status "accepted"@en ;
    skos:broader eu-rights:T4-SolidarityImpact ;
    skos:definition "Something that acts as or is considered as an impact on A32 Prohibition Of Child Labour Protectionof Young At Work"@en ;
    skos:inScheme eu-rights:impacts-classes ;
    skos:prefLabel "Impact on A32 Prohibition Of Child Labour Protectionof Young At Work"@en .

eu-rights:A33-FamilyProfessionalLifeImpact a rdfs:Class,
        skos:Concept,
        dpv:RiskConcept,
        risk:PotentialConsequence,
        risk:PotentialImpact,
        risk:PotentialRisk ;
    dct:contributor _:N0a43dd9ea5e94fe695d8b7df8802cfdd ;
    dct:created "2022-07-29"^^xsd:date ;
    dct:source [ a schema:WebPage ;
            schema:name "Charter of Fundamental Rights of the European Union" ;
            schema:url "http://data.europa.eu/eli/treaty/char_2012/oj" ] ;
    rdfs:isDefinedBy eu-rights: ;
    sw:term_status "accepted"@en ;
    skos:broader eu-rights:T4-SolidarityImpact ;
    skos:definition "Something that acts as or is considered as an impact on A33 Family Professional Life"@en ;
    skos:inScheme eu-rights:impacts-classes ;
    skos:prefLabel "Impact on A33 Family Professional Life"@en .

eu-rights:A34-SocialSecuritySocialAssistanceImpact a rdfs:Class,
        skos:Concept,
        dpv:RiskConcept,
        risk:PotentialConsequence,
        risk:PotentialImpact,
        risk:PotentialRisk ;
    dct:contributor _:N0a43dd9ea5e94fe695d8b7df8802cfdd ;
    dct:created "2022-07-30"^^xsd:date ;
    dct:source [ a schema:WebPage ;
            schema:name "Charter of Fundamental Rights of the European Union" ;
            schema:url "http://data.europa.eu/eli/treaty/char_2012/oj" ] ;
    rdfs:isDefinedBy eu-rights: ;
    sw:term_status "accepted"@en ;
    skos:broader eu-rights:T4-SolidarityImpact ;
    skos:definition "Something that acts as or is considered as an impact on A34 Social Security Social Assistance"@en ;
    skos:inScheme eu-rights:impacts-classes ;
    skos:prefLabel "Impact on A34 Social Security Social Assistance"@en .

eu-rights:A35-HealthcareImpact a rdfs:Class,
        skos:Concept,
        dpv:RiskConcept,
        risk:PotentialConsequence,
        risk:PotentialImpact,
        risk:PotentialRisk ;
    dct:contributor _:N0a43dd9ea5e94fe695d8b7df8802cfdd ;
    dct:created "2022-07-31"^^xsd:date ;
    dct:source [ a schema:WebPage ;
            schema:name "Charter of Fundamental Rights of the European Union" ;
            schema:url "http://data.europa.eu/eli/treaty/char_2012/oj" ] ;
    rdfs:isDefinedBy eu-rights: ;
    sw:term_status "accepted"@en ;
    skos:broader eu-rights:T4-SolidarityImpact ;
    skos:definition "Something that acts as or is considered as an impact on A35 Healthcare"@en ;
    skos:inScheme eu-rights:impacts-classes ;
    skos:prefLabel "Impact on A35 Healthcare"@en .

eu-rights:A36-AccessToServicesOfGeneralEconomicInterestImpact a rdfs:Class,
        skos:Concept,
        dpv:RiskConcept,
        risk:PotentialConsequence,
        risk:PotentialImpact,
        risk:PotentialRisk ;
    dct:contributor _:N0a43dd9ea5e94fe695d8b7df8802cfdd ;
    dct:created "2022-08-01"^^xsd:date ;
    dct:source [ a schema:WebPage ;
            schema:name "Charter of Fundamental Rights of the European Union" ;
            schema:url "http://data.europa.eu/eli/treaty/char_2012/oj" ] ;
    rdfs:isDefinedBy eu-rights: ;
    sw:term_status "accepted"@en ;
    skos:broader eu-rights:T4-SolidarityImpact ;
    skos:definition "Something that acts as or is considered as an impact on A36 Access To Services Of General Economic Interest"@en ;
    skos:inScheme eu-rights:impacts-classes ;
    skos:prefLabel "Impact on A36 Access To Services Of General Economic Interest"@en .

eu-rights:A37-EnvironmentalProtectionImpact a rdfs:Class,
        skos:Concept,
        dpv:RiskConcept,
        risk:PotentialConsequence,
        risk:PotentialImpact,
        risk:PotentialRisk ;
    dct:contributor _:N0a43dd9ea5e94fe695d8b7df8802cfdd ;
    dct:created "2022-08-02"^^xsd:date ;
    dct:source [ a schema:WebPage ;
            schema:name "Charter of Fundamental Rights of the European Union" ;
            schema:url "http://data.europa.eu/eli/treaty/char_2012/oj" ] ;
    rdfs:isDefinedBy eu-rights: ;
    sw:term_status "accepted"@en ;
    skos:broader eu-rights:T4-SolidarityImpact ;
    skos:definition "Something that acts as or is considered as an impact on A37 Environmental Protection"@en ;
    skos:inScheme eu-rights:impacts-classes ;
    skos:prefLabel "Impact on A37 Environmental Protection"@en .

eu-rights:A38-ConsumerProtectionImpact a rdfs:Class,
        skos:Concept,
        dpv:RiskConcept,
        risk:PotentialConsequence,
        risk:PotentialImpact,
        risk:PotentialRisk ;
    dct:contributor _:N0a43dd9ea5e94fe695d8b7df8802cfdd ;
    dct:created "2022-08-03"^^xsd:date ;
    dct:source [ a schema:WebPage ;
            schema:name "Charter of Fundamental Rights of the European Union" ;
            schema:url "http://data.europa.eu/eli/treaty/char_2012/oj" ] ;
    rdfs:isDefinedBy eu-rights: ;
    sw:term_status "accepted"@en ;
    skos:broader eu-rights:T4-SolidarityImpact ;
    skos:definition "Something that acts as or is considered as an impact on A38 Consumer Protection"@en ;
    skos:inScheme eu-rights:impacts-classes ;
    skos:prefLabel "Impact on A38 Consumer Protection"@en .

eu-rights:A39-RightToVoteStandAsCanditateEUParliamentImpact a rdfs:Class,
        skos:Concept,
        dpv:RiskConcept,
        risk:PotentialConsequence,
        risk:PotentialImpact,
        risk:PotentialRisk ;
    dct:contributor _:N0a43dd9ea5e94fe695d8b7df8802cfdd ;
    dct:created "2022-08-05"^^xsd:date ;
    dct:source [ a schema:WebPage ;
            schema:name "Charter of Fundamental Rights of the European Union" ;
            schema:url "http://data.europa.eu/eli/treaty/char_2012/oj" ] ;
    rdfs:isDefinedBy eu-rights: ;
    sw:term_status "accepted"@en ;
    skos:broader eu-rights:T5-CitizensRightsImpact ;
    skos:definition "Something that acts as or is considered as an impact on A39 Right To Vote Stand As Candidate E U Parliament"@en ;
    skos:inScheme eu-rights:impacts-classes ;
    skos:prefLabel "Impact on A39 Right To Vote Stand As Candidate E U Parliament"@en .

eu-rights:A4-ProhibitionOfTortureDegradationPunishmentImpact a rdfs:Class,
        skos:Concept,
        dpv:RiskConcept,
        risk:PotentialConsequence,
        risk:PotentialImpact,
        risk:PotentialRisk ;
    dct:contributor _:N0a43dd9ea5e94fe695d8b7df8802cfdd ;
    dct:created "2022-06-27"^^xsd:date ;
    dct:source [ a schema:WebPage ;
            schema:name "Charter of Fundamental Rights of the European Union" ;
            schema:url "http://data.europa.eu/eli/treaty/char_2012/oj" ] ;
    rdfs:isDefinedBy eu-rights: ;
    sw:term_status "accepted"@en ;
    skos:broader eu-rights:T1-DignityImpact ;
    skos:definition "Something that acts as or is considered as an impact on A4 Prohibition Of Torture Degradation Punishment"@en ;
    skos:inScheme eu-rights:impacts-classes ;
    skos:prefLabel "Impact on A4 Prohibition Of Torture Degradation Punishment"@en .

eu-rights:A40-RightToVoteStandAsCandidateMunicipalElectionsImpact a rdfs:Class,
        skos:Concept,
        dpv:RiskConcept,
        risk:PotentialConsequence,
        risk:PotentialImpact,
        risk:PotentialRisk ;
    dct:contributor _:N0a43dd9ea5e94fe695d8b7df8802cfdd ;
    dct:created "2022-08-06"^^xsd:date ;
    dct:source [ a schema:WebPage ;
            schema:name "Charter of Fundamental Rights of the European Union" ;
            schema:url "http://data.europa.eu/eli/treaty/char_2012/oj" ] ;
    rdfs:isDefinedBy eu-rights: ;
    sw:term_status "accepted"@en ;
    skos:broader eu-rights:T5-CitizensRightsImpact ;
    skos:definition "Something that acts as or is considered as an impact on A40 Right To Vote Stand As Candidate Municipal Elections"@en ;
    skos:inScheme eu-rights:impacts-classes ;
    skos:prefLabel "Impact on A40 Right To Vote Stand As Candidate Municipal Elections"@en .

eu-rights:A41-RightToGoodAdministrationImpact a rdfs:Class,
        skos:Concept,
        dpv:RiskConcept,
        risk:PotentialConsequence,
        risk:PotentialImpact,
        risk:PotentialRisk ;
    dct:contributor _:N0a43dd9ea5e94fe695d8b7df8802cfdd ;
    dct:created "2022-08-07"^^xsd:date ;
    dct:source [ a schema:WebPage ;
            schema:name "Charter of Fundamental Rights of the European Union" ;
            schema:url "http://data.europa.eu/eli/treaty/char_2012/oj" ] ;
    rdfs:isDefinedBy eu-rights: ;
    sw:term_status "accepted"@en ;
    skos:broader eu-rights:T5-CitizensRightsImpact ;
    skos:definition "Something that acts as or is considered as an impact on A41 Right To Good Administration"@en ;
    skos:inScheme eu-rights:impacts-classes ;
    skos:prefLabel "Impact on A41 Right To Good Administration"@en .

eu-rights:A42-RightToAccessToDocumentsImpact a rdfs:Class,
        skos:Concept,
        dpv:RiskConcept,
        risk:PotentialConsequence,
        risk:PotentialImpact,
        risk:PotentialRisk ;
    dct:contributor _:N0a43dd9ea5e94fe695d8b7df8802cfdd ;
    dct:created "2022-08-08"^^xsd:date ;
    dct:source [ a schema:WebPage ;
            schema:name "Charter of Fundamental Rights of the European Union" ;
            schema:url "http://data.europa.eu/eli/treaty/char_2012/oj" ] ;
    rdfs:isDefinedBy eu-rights: ;
    sw:term_status "accepted"@en ;
    skos:broader eu-rights:T5-CitizensRightsImpact ;
    skos:definition "Something that acts as or is considered as an impact on A42 Right To Access To Documents"@en ;
    skos:inScheme eu-rights:impacts-classes ;
    skos:prefLabel "Impact on A42 Right To Access To Documents"@en .

eu-rights:A43-EuropeanOmbudsmanImpact a rdfs:Class,
        skos:Concept,
        dpv:RiskConcept,
        risk:PotentialConsequence,
        risk:PotentialImpact,
        risk:PotentialRisk ;
    dct:contributor _:N0a43dd9ea5e94fe695d8b7df8802cfdd ;
    dct:created "2022-08-09"^^xsd:date ;
    dct:source [ a schema:WebPage ;
            schema:name "Charter of Fundamental Rights of the European Union" ;
            schema:url "http://data.europa.eu/eli/treaty/char_2012/oj" ] ;
    rdfs:isDefinedBy eu-rights: ;
    sw:term_status "accepted"@en ;
    skos:broader eu-rights:T5-CitizensRightsImpact ;
    skos:definition "Something that acts as or is considered as an impact on A43 European Ombudsman"@en ;
    skos:inScheme eu-rights:impacts-classes ;
    skos:prefLabel "Impact on A43 European Ombudsman"@en .

eu-rights:A44-RightToPetitionImpact a rdfs:Class,
        skos:Concept,
        dpv:RiskConcept,
        risk:PotentialConsequence,
        risk:PotentialImpact,
        risk:PotentialRisk ;
    dct:contributor _:N0a43dd9ea5e94fe695d8b7df8802cfdd ;
    dct:created "2022-08-10"^^xsd:date ;
    dct:source [ a schema:WebPage ;
            schema:name "Charter of Fundamental Rights of the European Union" ;
            schema:url "http://data.europa.eu/eli/treaty/char_2012/oj" ] ;
    rdfs:isDefinedBy eu-rights: ;
    sw:term_status "accepted"@en ;
    skos:broader eu-rights:T5-CitizensRightsImpact ;
    skos:definition "Something that acts as or is considered as an impact on A44 Right To Petition"@en ;
    skos:inScheme eu-rights:impacts-classes ;
    skos:prefLabel "Impact on A44 Right To Petition"@en .

eu-rights:A45-FreedomOfMovementAndResidenceImpact a rdfs:Class,
        skos:Concept,
        dpv:RiskConcept,
        risk:PotentialConsequence,
        risk:PotentialImpact,
        risk:PotentialRisk ;
    dct:contributor _:N0a43dd9ea5e94fe695d8b7df8802cfdd ;
    dct:created "2022-08-11"^^xsd:date ;
    dct:source [ a schema:WebPage ;
            schema:name "Charter of Fundamental Rights of the European Union" ;
            schema:url "http://data.europa.eu/eli/treaty/char_2012/oj" ] ;
    rdfs:isDefinedBy eu-rights: ;
    sw:term_status "accepted"@en ;
    skos:broader eu-rights:T5-CitizensRightsImpact ;
    skos:definition "Something that acts as or is considered as an impact on A45 Freedom Of Movement And Residence"@en ;
    skos:inScheme eu-rights:impacts-classes ;
    skos:prefLabel "Impact on A45 Freedom Of Movement And Residence"@en .

eu-rights:A46-DiplomaticConsularProtectionImpact a rdfs:Class,
        skos:Concept,
        dpv:RiskConcept,
        risk:PotentialConsequence,
        risk:PotentialImpact,
        risk:PotentialRisk ;
    dct:contributor _:N0a43dd9ea5e94fe695d8b7df8802cfdd ;
    dct:created "2022-08-12"^^xsd:date ;
    dct:source [ a schema:WebPage ;
            schema:name "Charter of Fundamental Rights of the European Union" ;
            schema:url "http://data.europa.eu/eli/treaty/char_2012/oj" ] ;
    rdfs:isDefinedBy eu-rights: ;
    sw:term_status "accepted"@en ;
    skos:broader eu-rights:T5-CitizensRightsImpact ;
    skos:definition "Something that acts as or is considered as an impact on A46 Diplomatic Consular Protection"@en ;
    skos:inScheme eu-rights:impacts-classes ;
    skos:prefLabel "Impact on A46 Diplomatic Consular Protection"@en .

eu-rights:A47-RightToEffectiveRemedyFairTrialImpact a rdfs:Class,
        skos:Concept,
        dpv:RiskConcept,
        risk:PotentialConsequence,
        risk:PotentialImpact,
        risk:PotentialRisk ;
    dct:contributor _:N0a43dd9ea5e94fe695d8b7df8802cfdd ;
    dct:created "2022-08-14"^^xsd:date ;
    dct:source [ a schema:WebPage ;
            schema:name "Charter of Fundamental Rights of the European Union" ;
            schema:url "http://data.europa.eu/eli/treaty/char_2012/oj" ] ;
    rdfs:isDefinedBy eu-rights: ;
    sw:term_status "accepted"@en ;
    skos:broader eu-rights:T6-JusticeImpact ;
    skos:definition "Something that acts as or is considered as an impact on A47 Right To Effective Remedy Fair Trial"@en ;
    skos:inScheme eu-rights:impacts-classes ;
    skos:prefLabel "Impact on A47 Right To Effective Remedy Fair Trial"@en .

eu-rights:A48-PresumptionOfInnocenceRightOfDefenceImpact a rdfs:Class,
        skos:Concept,
        dpv:RiskConcept,
        risk:PotentialConsequence,
        risk:PotentialImpact,
        risk:PotentialRisk ;
    dct:contributor _:N0a43dd9ea5e94fe695d8b7df8802cfdd ;
    dct:created "2022-08-15"^^xsd:date ;
    dct:source [ a schema:WebPage ;
            schema:name "Charter of Fundamental Rights of the European Union" ;
            schema:url "http://data.europa.eu/eli/treaty/char_2012/oj" ] ;
    rdfs:isDefinedBy eu-rights: ;
    sw:term_status "accepted"@en ;
    skos:broader eu-rights:T6-JusticeImpact ;
    skos:definition "Something that acts as or is considered as an impact on A48 Presumption Of Innocence Right Of Defence"@en ;
    skos:inScheme eu-rights:impacts-classes ;
    skos:prefLabel "Impact on A48 Presumption Of Innocence Right Of Defence"@en .

eu-rights:A49-PrinciplesOfLegalityProportionalityCriminalOffencesPenaltiesImpact a rdfs:Class,
        skos:Concept,
        dpv:RiskConcept,
        risk:PotentialConsequence,
        risk:PotentialImpact,
        risk:PotentialRisk ;
    dct:contributor _:N0a43dd9ea5e94fe695d8b7df8802cfdd ;
    dct:created "2022-08-16"^^xsd:date ;
    dct:source [ a schema:WebPage ;
            schema:name "Charter of Fundamental Rights of the European Union" ;
            schema:url "http://data.europa.eu/eli/treaty/char_2012/oj" ] ;
    rdfs:isDefinedBy eu-rights: ;
    sw:term_status "accepted"@en ;
    skos:broader eu-rights:T6-JusticeImpact ;
    skos:definition "Something that acts as or is considered as an impact on A49 Principles Of Legality Proportionality Criminal Offences Penalties"@en ;
    skos:inScheme eu-rights:impacts-classes ;
    skos:prefLabel "Impact on A49 Principles Of Legality Proportionality Criminal Offences Penalties"@en .

eu-rights:A5-ProhibitionOfSlaveryForcedLabourImpact a rdfs:Class,
        skos:Concept,
        dpv:RiskConcept,
        risk:PotentialConsequence,
        risk:PotentialImpact,
        risk:PotentialRisk ;
    dct:contributor _:N0a43dd9ea5e94fe695d8b7df8802cfdd ;
    dct:created "2022-06-28"^^xsd:date ;
    dct:source [ a schema:WebPage ;
            schema:name "Charter of Fundamental Rights of the European Union" ;
            schema:url "http://data.europa.eu/eli/treaty/char_2012/oj" ] ;
    rdfs:isDefinedBy eu-rights: ;
    sw:term_status "accepted"@en ;
    skos:broader eu-rights:T1-DignityImpact ;
    skos:definition "Something that acts as or is considered as an impact on A5 Prohibition Of Slavery Forced Labour"@en ;
    skos:inScheme eu-rights:impacts-classes ;
    skos:prefLabel "Impact on A5 Prohibition Of Slavery Forced Labour"@en .

eu-rights:A50-RightNotBeTriedPunishedTwiceForSameCriminalOffenceImpact a rdfs:Class,
        skos:Concept,
        dpv:RiskConcept,
        risk:PotentialConsequence,
        risk:PotentialImpact,
        risk:PotentialRisk ;
    dct:contributor _:N0a43dd9ea5e94fe695d8b7df8802cfdd ;
    dct:created "2022-08-17"^^xsd:date ;
    dct:source [ a schema:WebPage ;
            schema:name "Charter of Fundamental Rights of the European Union" ;
            schema:url "http://data.europa.eu/eli/treaty/char_2012/oj" ] ;
    rdfs:isDefinedBy eu-rights: ;
    sw:term_status "accepted"@en ;
    skos:broader eu-rights:T6-JusticeImpact ;
    skos:definition "Something that acts as or is considered as an impact on A50 Right Not Be Tried Punished Twice For Same Criminal Offence"@en ;
    skos:inScheme eu-rights:impacts-classes ;
    skos:prefLabel "Impact on A50 Right Not Be Tried Punished Twice For Same Criminal Offence"@en .

eu-rights:A51-FieldOfApplicationImpact a rdfs:Class,
        skos:Concept,
        dpv:RiskConcept,
        risk:PotentialConsequence,
        risk:PotentialImpact,
        risk:PotentialRisk ;
    dct:contributor _:N0a43dd9ea5e94fe695d8b7df8802cfdd ;
    dct:created "2022-08-19"^^xsd:date ;
    dct:source [ a schema:WebPage ;
            schema:name "Charter of Fundamental Rights of the European Union" ;
            schema:url "http://data.europa.eu/eli/treaty/char_2012/oj" ] ;
    rdfs:isDefinedBy eu-rights: ;
    sw:term_status "accepted"@en ;
    skos:broader eu-rights:T7-InterpretationAndApplicationImpact ;
    skos:definition "Something that acts as or is considered as an impact on A51 Field Of Application"@en ;
    skos:inScheme eu-rights:impacts-classes ;
    skos:prefLabel "Impact on A51 Field Of Application"@en .

eu-rights:A52-ScopeInterpretationOfRightsPrinciplesImpact a rdfs:Class,
        skos:Concept,
        dpv:RiskConcept,
        risk:PotentialConsequence,
        risk:PotentialImpact,
        risk:PotentialRisk ;
    dct:contributor _:N0a43dd9ea5e94fe695d8b7df8802cfdd ;
    dct:created "2022-08-20"^^xsd:date ;
    dct:source [ a schema:WebPage ;
            schema:name "Charter of Fundamental Rights of the European Union" ;
            schema:url "http://data.europa.eu/eli/treaty/char_2012/oj" ] ;
    rdfs:isDefinedBy eu-rights: ;
    sw:term_status "accepted"@en ;
    skos:broader eu-rights:T7-InterpretationAndApplicationImpact ;
    skos:definition "Something that acts as or is considered as an impact on A52 Scope Interpretation Of Rights Principles"@en ;
    skos:inScheme eu-rights:impacts-classes ;
    skos:prefLabel "Impact on A52 Scope Interpretation Of Rights Principles"@en .

eu-rights:A53-LevelOfProtectionImpact a rdfs:Class,
        skos:Concept,
        dpv:RiskConcept,
        risk:PotentialConsequence,
        risk:PotentialImpact,
        risk:PotentialRisk ;
    dct:contributor _:N0a43dd9ea5e94fe695d8b7df8802cfdd ;
    dct:created "2022-08-21"^^xsd:date ;
    dct:source [ a schema:WebPage ;
            schema:name "Charter of Fundamental Rights of the European Union" ;
            schema:url "http://data.europa.eu/eli/treaty/char_2012/oj" ] ;
    rdfs:isDefinedBy eu-rights: ;
    sw:term_status "accepted"@en ;
    skos:broader eu-rights:T7-InterpretationAndApplicationImpact ;
    skos:definition "Something that acts as or is considered as an impact on A53 Level Of Protection"@en ;
    skos:inScheme eu-rights:impacts-classes ;
    skos:prefLabel "Impact on A53 Level Of Protection"@en .

eu-rights:A54-ProhibitionOfAbuseOfRightsImpact a rdfs:Class,
        skos:Concept,
        dpv:RiskConcept,
        risk:PotentialConsequence,
        risk:PotentialImpact,
        risk:PotentialRisk ;
    dct:contributor _:N0a43dd9ea5e94fe695d8b7df8802cfdd ;
    dct:created "2022-08-22"^^xsd:date ;
    dct:source [ a schema:WebPage ;
            schema:name "Charter of Fundamental Rights of the European Union" ;
            schema:url "http://data.europa.eu/eli/treaty/char_2012/oj" ] ;
    rdfs:isDefinedBy eu-rights: ;
    sw:term_status "accepted"@en ;
    skos:broader eu-rights:T7-InterpretationAndApplicationImpact ;
    skos:definition "Something that acts as or is considered as an impact on A54 Prohibition Of Abuse Of Rights"@en ;
    skos:inScheme eu-rights:impacts-classes ;
    skos:prefLabel "Impact on A54 Prohibition Of Abuse Of Rights"@en .

eu-rights:A6-RightToLiberySecurityImpact a rdfs:Class,
        skos:Concept,
        dpv:RiskConcept,
        risk:PotentialConsequence,
        risk:PotentialImpact,
        risk:PotentialRisk ;
    dct:contributor _:N0a43dd9ea5e94fe695d8b7df8802cfdd ;
    dct:created "2022-06-30"^^xsd:date ;
    dct:source [ a schema:WebPage ;
            schema:name "Charter of Fundamental Rights of the European Union" ;
            schema:url "http://data.europa.eu/eli/treaty/char_2012/oj" ] ;
    rdfs:isDefinedBy eu-rights: ;
    sw:term_status "accepted"@en ;
    skos:broader eu-rights:T2-FreedomsImpact ;
    skos:definition "Something that acts as or is considered as an impact on A6 Right To Liberty Security"@en ;
    skos:inScheme eu-rights:impacts-classes ;
    skos:prefLabel "Impact on A6 Right To Liberty Security"@en .

eu-rights:A7-RespectPrivateFamilyLifeImpact a rdfs:Class,
        skos:Concept,
        dpv:RiskConcept,
        risk:PotentialConsequence,
        risk:PotentialImpact,
        risk:PotentialRisk ;
    dct:contributor _:N0a43dd9ea5e94fe695d8b7df8802cfdd ;
    dct:created "2022-07-01"^^xsd:date ;
    dct:source [ a schema:WebPage ;
            schema:name "Charter of Fundamental Rights of the European Union" ;
            schema:url "http://data.europa.eu/eli/treaty/char_2012/oj" ] ;
    rdfs:isDefinedBy eu-rights: ;
    sw:term_status "accepted"@en ;
    skos:broader eu-rights:T2-FreedomsImpact ;
    skos:definition "Something that acts as or is considered as an impact on A7 Respect Private Family Life"@en ;
    skos:inScheme eu-rights:impacts-classes ;
    skos:prefLabel "Impact on A7 Respect Private Family Life"@en .

eu-rights:A8-AccessImpacted a rdfs:Class,
        skos:Concept,
        dpv:RiskConcept,
        risk:PotentialConsequence,
        risk:PotentialImpact,
        risk:PotentialRisk ;
    dct:created "2024-10-22"^^xsd:date ;
    dct:source [ a schema:WebPage ;
            schema:name "Charter of Fundamental Rights of the European Union" ;
            schema:url "http://data.europa.eu/eli/treaty/char_2012/oj" ] ;
    rdfs:isDefinedBy eu-rights: ;
    sw:term_status "accepted"@en ;
    skos:broader eu-rights:A8-ProtectionOfPersonalDataImpact ;
    skos:definition "Where the right of access of personal data is impacted"@en ;
    skos:inScheme eu-rights:impacts-classes ;
    skos:prefLabel "A8 Access Impacted"@en ;
    skos:scopeNote "This concept is experimental and may change in future versions"@en .

eu-rights:A8-Denied a rdfs:Class,
        skos:Concept,
        dpv:RiskConcept,
        risk:PotentialConsequence,
        risk:PotentialImpact,
        risk:PotentialRisk ;
    dct:created "2024-10-22"^^xsd:date ;
    dct:source [ a schema:WebPage ;
            schema:name "Charter of Fundamental Rights of the European Union" ;
            schema:url "http://data.europa.eu/eli/treaty/char_2012/oj" ] ;
    rdfs:isDefinedBy eu-rights: ;
    sw:term_status "accepted"@en ;
    skos:broader eu-rights:A8-ProtectionOfPersonalDataImpact ;
    skos:definition "Where the protection of personal data is denied to be applicable or required"@en ;
    skos:inScheme eu-rights:impacts-classes ;
    skos:prefLabel "A8 Denied"@en ;
    skos:scopeNote "This concept is experimental and may change in future versions"@en .

eu-rights:A8-Eroded a rdfs:Class,
        skos:Concept,
        dpv:RiskConcept,
        risk:PotentialConsequence,
        risk:PotentialImpact,
        risk:PotentialRisk ;
    dct:created "2024-10-22"^^xsd:date ;
    dct:source [ a schema:WebPage ;
            schema:name "Charter of Fundamental Rights of the European Union" ;
            schema:url "http://data.europa.eu/eli/treaty/char_2012/oj" ] ;
    rdfs:isDefinedBy eu-rights: ;
    sw:term_status "accepted"@en ;
    skos:broader eu-rights:A8-ProtectionOfPersonalDataImpact ;
    skos:definition "Where the protection of personal data is affected negatively systematically and over time"@en ;
    skos:inScheme eu-rights:impacts-classes ;
    skos:prefLabel "A8 Eroded"@en ;
    skos:scopeNote "This concept is experimental and may change in future versions"@en .

eu-rights:A8-ExercisePrevented a rdfs:Class,
        skos:Concept,
        dpv:RiskConcept,
        risk:PotentialConsequence,
        risk:PotentialImpact,
        risk:PotentialRisk ;
    dct:created "2024-10-22"^^xsd:date ;
    dct:source [ a schema:WebPage ;
            schema:name "Charter of Fundamental Rights of the European Union" ;
            schema:url "http://data.europa.eu/eli/treaty/char_2012/oj" ] ;
    rdfs:isDefinedBy eu-rights: ;
    sw:term_status "accepted"@en ;
    skos:broader eu-rights:A8-ProtectionOfPersonalDataImpact ;
    skos:definition "Where the protection of personal data is prevented from being carried out"@en ;
    skos:inScheme eu-rights:impacts-classes ;
    skos:prefLabel "A8 ExercisePrevented"@en ;
    skos:scopeNote "This concept is experimental and may change in future versions"@en .

eu-rights:A8-Limited a rdfs:Class,
        skos:Concept,
        dpv:RiskConcept,
        risk:PotentialConsequence,
        risk:PotentialImpact,
        risk:PotentialRisk ;
    dct:created "2024-10-22"^^xsd:date ;
    dct:source [ a schema:WebPage ;
            schema:name "Charter of Fundamental Rights of the European Union" ;
            schema:url "http://data.europa.eu/eli/treaty/char_2012/oj" ] ;
    rdfs:isDefinedBy eu-rights: ;
    sw:term_status "accepted"@en ;
    skos:broader eu-rights:A8-ProtectionOfPersonalDataImpact ;
    skos:definition "Where not all personal data has been protected or adequately protected"@en ;
    skos:inScheme eu-rights:impacts-classes ;
    skos:prefLabel "A8 Limited"@en ;
    skos:scopeNote "This concept is experimental and may change in future versions"@en .

eu-rights:A8-Obstructed a rdfs:Class,
        skos:Concept,
        dpv:RiskConcept,
        risk:PotentialConsequence,
        risk:PotentialImpact,
        risk:PotentialRisk ;
    dct:created "2024-10-22"^^xsd:date ;
    dct:source [ a schema:WebPage ;
            schema:name "Charter of Fundamental Rights of the European Union" ;
            schema:url "http://data.europa.eu/eli/treaty/char_2012/oj" ] ;
    rdfs:isDefinedBy eu-rights: ;
    sw:term_status "accepted"@en ;
    skos:broader eu-rights:A8-ProtectionOfPersonalDataImpact ;
    skos:definition "Where barriers are created or are present to protect personal data"@en ;
    skos:inScheme eu-rights:impacts-classes ;
    skos:prefLabel "A8 Obstructed"@en ;
    skos:scopeNote "This concept is experimental and may change in future versions"@en .

eu-rights:A8-ProcessingWithNonspecificPurposes a rdfs:Class,
        skos:Concept,
        dpv:RiskConcept,
        risk:PotentialConsequence,
        risk:PotentialImpact,
        risk:PotentialRisk ;
    dct:created "2024-10-22"^^xsd:date ;
    dct:source [ a schema:WebPage ;
            schema:name "Charter of Fundamental Rights of the European Union" ;
            schema:url "http://data.europa.eu/eli/treaty/char_2012/oj" ] ;
    rdfs:isDefinedBy eu-rights: ;
    sw:term_status "accepted"@en ;
    skos:broader eu-rights:A8-ProtectionOfPersonalDataImpact ;
    skos:definition "Where there is processing of personal data for or with non-specific purposes i.e. processing is not limited to specific purposes"@en ;
    skos:inScheme eu-rights:impacts-classes ;
    skos:prefLabel "A8 Processing with Nonspecific Purposes"@en ;
    skos:scopeNote "This concept is experimental and may change in future versions"@en .

eu-rights:A8-ProcessingWithoutValidConsent a rdfs:Class,
        skos:Concept,
        dpv:RiskConcept,
        risk:PotentialConsequence,
        risk:PotentialImpact,
        risk:PotentialRisk ;
    dct:created "2024-10-22"^^xsd:date ;
    dct:source [ a schema:WebPage ;
            schema:name "Charter of Fundamental Rights of the European Union" ;
            schema:url "http://data.europa.eu/eli/treaty/char_2012/oj" ] ;
    rdfs:isDefinedBy eu-rights: ;
    sw:term_status "accepted"@en ;
    skos:broader eu-rights:A8-ProtectionOfPersonalDataImpact ;
    skos:definition "Where there is processing of personal data without valid consent where consent is the valid legal basis as established in law"@en ;
    skos:inScheme eu-rights:impacts-classes ;
    skos:prefLabel "A8 Processing without Valid Consent"@en ;
    skos:scopeNote "This concept is experimental and may change in future versions"@en .

eu-rights:A8-ProcessingWithoutValidLegalBasis a rdfs:Class,
        skos:Concept,
        dpv:RiskConcept,
        risk:PotentialConsequence,
        risk:PotentialImpact,
        risk:PotentialRisk ;
    dct:created "2024-10-22"^^xsd:date ;
    dct:source [ a schema:WebPage ;
            schema:name "Charter of Fundamental Rights of the European Union" ;
            schema:url "http://data.europa.eu/eli/treaty/char_2012/oj" ] ;
    rdfs:isDefinedBy eu-rights: ;
    sw:term_status "accepted"@en ;
    skos:broader eu-rights:A8-ProtectionOfPersonalDataImpact ;
    skos:definition "Where there is processing of personal data without a valid legal basis established in law"@en ;
    skos:inScheme eu-rights:impacts-classes ;
    skos:prefLabel "A8 Processing without Valid Legal Basis"@en ;
    skos:scopeNote "This concept is experimental and may change in future versions"@en .

eu-rights:A8-ProtectionOfPersonalDataImpact a rdfs:Class,
        skos:Concept,
        dpv:RiskConcept,
        risk:PotentialConsequence,
        risk:PotentialImpact,
        risk:PotentialRisk ;
    dct:contributor _:N0a43dd9ea5e94fe695d8b7df8802cfdd ;
    dct:created "2022-07-02"^^xsd:date ;
    dct:source [ a schema:WebPage ;
            schema:name "Charter of Fundamental Rights of the European Union" ;
            schema:url "http://data.europa.eu/eli/treaty/char_2012/oj" ] ;
    rdfs:isDefinedBy eu-rights: ;
    sw:term_status "accepted"@en ;
    skos:broader eu-rights:T2-FreedomsImpact ;
    skos:definition "Something that acts as or is considered as an impact on A8 Protection Of Personal Data"@en ;
    skos:inScheme eu-rights:impacts-classes ;
    skos:prefLabel "Impact on A8 Protection Of Personal Data"@en .

eu-rights:A8-RectificiationImpacted a rdfs:Class,
        skos:Concept,
        dpv:RiskConcept,
        risk:PotentialConsequence,
        risk:PotentialImpact,
        risk:PotentialRisk ;
    dct:created "2024-10-22"^^xsd:date ;
    dct:source [ a schema:WebPage ;
            schema:name "Charter of Fundamental Rights of the European Union" ;
            schema:url "http://data.europa.eu/eli/treaty/char_2012/oj" ] ;
    rdfs:isDefinedBy eu-rights: ;
    sw:term_status "accepted"@en ;
    skos:broader eu-rights:A8-ProtectionOfPersonalDataImpact ;
    skos:definition "Where the right of rectification of personal data is impacted"@en ;
    skos:inScheme eu-rights:impacts-classes ;
    skos:prefLabel "A8 Rectificiation Impacted"@en ;
    skos:scopeNote "This concept is experimental and may change in future versions"@en .

eu-rights:A8-UnfairProcessing a rdfs:Class,
        skos:Concept,
        dpv:RiskConcept,
        risk:PotentialConsequence,
        risk:PotentialImpact,
        risk:PotentialRisk ;
    dct:created "2024-10-22"^^xsd:date ;
    dct:source [ a schema:WebPage ;
            schema:name "Charter of Fundamental Rights of the European Union" ;
            schema:url "http://data.europa.eu/eli/treaty/char_2012/oj" ] ;
    rdfs:isDefinedBy eu-rights: ;
    sw:term_status "accepted"@en ;
    skos:broader eu-rights:A8-ProtectionOfPersonalDataImpact ;
    skos:definition "Where there is unfair processing of personal data"@en ;
    skos:inScheme eu-rights:impacts-classes ;
    skos:prefLabel "A8 Unfair Processing"@en ;
    skos:scopeNote "This concept is experimental and may change in future versions"@en .

eu-rights:A8-Unfulfilled a rdfs:Class,
        skos:Concept,
        dpv:RiskConcept,
        risk:PotentialConsequence,
        risk:PotentialImpact,
        risk:PotentialRisk ;
    dct:created "2024-10-22"^^xsd:date ;
    dct:source [ a schema:WebPage ;
            schema:name "Charter of Fundamental Rights of the European Union" ;
            schema:url "http://data.europa.eu/eli/treaty/char_2012/oj" ] ;
    rdfs:isDefinedBy eu-rights: ;
    sw:term_status "accepted"@en ;
    skos:broader eu-rights:A8-ProtectionOfPersonalDataImpact ;
    skos:definition "Where the protection of personal data is not carried out"@en ;
    skos:inScheme eu-rights:impacts-classes ;
    skos:prefLabel "A8 Unfulfilled"@en ;
    skos:scopeNote "This concept is experimental and may change in future versions"@en .

eu-rights:A8-Violated a rdfs:Class,
        skos:Concept,
        dpv:RiskConcept,
        risk:PotentialConsequence,
        risk:PotentialImpact,
        risk:PotentialRisk ;
    dct:created "2024-10-22"^^xsd:date ;
    dct:source [ a schema:WebPage ;
            schema:name "Charter of Fundamental Rights of the European Union" ;
            schema:url "http://data.europa.eu/eli/treaty/char_2012/oj" ] ;
    rdfs:isDefinedBy eu-rights: ;
    sw:term_status "accepted"@en ;
    skos:broader eu-rights:A8-ProtectionOfPersonalDataImpact ;
    skos:definition "Where the right to protection of personal data is violated"@en ;
    skos:inScheme eu-rights:impacts-classes ;
    skos:prefLabel "A8 Violated"@en ;
    skos:scopeNote "This concept is experimental and may change in future versions"@en .

eu-rights:A9-RightToMarryFoundFamilyImpact a rdfs:Class,
        skos:Concept,
        dpv:RiskConcept,
        risk:PotentialConsequence,
        risk:PotentialImpact,
        risk:PotentialRisk ;
    dct:contributor _:N0a43dd9ea5e94fe695d8b7df8802cfdd ;
    dct:created "2022-07-03"^^xsd:date ;
    dct:source [ a schema:WebPage ;
            schema:name "Charter of Fundamental Rights of the European Union" ;
            schema:url "http://data.europa.eu/eli/treaty/char_2012/oj" ] ;
    rdfs:isDefinedBy eu-rights: ;
    sw:term_status "accepted"@en ;
    skos:broader eu-rights:T2-FreedomsImpact ;
    skos:definition "Something that acts as or is considered as an impact on A9 Right To Marry Found Family"@en ;
    skos:inScheme eu-rights:impacts-classes ;
    skos:prefLabel "Impact on A9 Right To Marry Found Family"@en .

eu-rights:EUFundamentalRightsImpact a rdfs:Class,
        skos:Concept,
        dpv:RiskConcept,
        risk:PotentialConsequence,
        risk:PotentialImpact,
        risk:PotentialRisk ;
    dct:contributor _:N0a43dd9ea5e94fe695d8b7df8802cfdd ;
    dct:created "2022-06-22"^^xsd:date ;
    dct:source [ a schema:WebPage ;
            schema:name "Charter of Fundamental Rights of the European Union" ;
            schema:url "http://data.europa.eu/eli/treaty/char_2012/oj" ] ;
    rdfs:isDefinedBy eu-rights: ;
    sw:term_status "accepted"@en ;
    skos:broader risk:RightsImpact ;
    skos:definition "Something that acts as or is considered as an impact on EU Fundamental Rights"@en ;
    skos:inScheme eu-rights:impacts-classes ;
    skos:prefLabel "Impact on EU Fundamental Rights"@en .

eu-rights:T1-DignityImpact a rdfs:Class,
        skos:Concept,
        dpv:RiskConcept,
        risk:PotentialConsequence,
        risk:PotentialImpact,
        risk:PotentialRisk ;
    dct:contributor _:N0a43dd9ea5e94fe695d8b7df8802cfdd ;
    dct:created "2022-06-23"^^xsd:date ;
    dct:source [ a schema:WebPage ;
            schema:name "Charter of Fundamental Rights of the European Union" ;
            schema:url "http://data.europa.eu/eli/treaty/char_2012/oj" ] ;
    rdfs:isDefinedBy eu-rights: ;
    sw:term_status "accepted"@en ;
    skos:broader eu-rights:EUFundamentalRightsImpact ;
    skos:definition "Something that acts as or is considered as an impact on T1 Dignity"@en ;
    skos:inScheme eu-rights:impacts-classes ;
    skos:prefLabel "Impact on T1 Dignity"@en .

eu-rights:T2-FreedomsImpact a rdfs:Class,
        skos:Concept,
        dpv:RiskConcept,
        risk:PotentialConsequence,
        risk:PotentialImpact,
        risk:PotentialRisk ;
    dct:contributor _:N0a43dd9ea5e94fe695d8b7df8802cfdd ;
    dct:created "2022-06-29"^^xsd:date ;
    dct:source [ a schema:WebPage ;
            schema:name "Charter of Fundamental Rights of the European Union" ;
            schema:url "http://data.europa.eu/eli/treaty/char_2012/oj" ] ;
    rdfs:isDefinedBy eu-rights: ;
    sw:term_status "accepted"@en ;
    skos:broader eu-rights:EUFundamentalRightsImpact ;
    skos:definition "Something that acts as or is considered as an impact on T2 Freedoms"@en ;
    skos:inScheme eu-rights:impacts-classes ;
    skos:prefLabel "Impact on T2 Freedoms"@en .

eu-rights:T3-EqualityImpact a rdfs:Class,
        skos:Concept,
        dpv:RiskConcept,
        risk:PotentialConsequence,
        risk:PotentialImpact,
        risk:PotentialRisk ;
    dct:contributor _:N0a43dd9ea5e94fe695d8b7df8802cfdd ;
    dct:created "2022-07-14"^^xsd:date ;
    dct:source [ a schema:WebPage ;
            schema:name "Charter of Fundamental Rights of the European Union" ;
            schema:url "http://data.europa.eu/eli/treaty/char_2012/oj" ] ;
    rdfs:isDefinedBy eu-rights: ;
    sw:term_status "accepted"@en ;
    skos:broader eu-rights:EUFundamentalRightsImpact ;
    skos:definition "Something that acts as or is considered as an impact on T3 Equality"@en ;
    skos:inScheme eu-rights:impacts-classes ;
    skos:prefLabel "Impact on T3 Equality"@en .

eu-rights:T4-SolidarityImpact a rdfs:Class,
        skos:Concept,
        dpv:RiskConcept,
        risk:PotentialConsequence,
        risk:PotentialImpact,
        risk:PotentialRisk ;
    dct:contributor _:N0a43dd9ea5e94fe695d8b7df8802cfdd ;
    dct:created "2022-07-22"^^xsd:date ;
    dct:source [ a schema:WebPage ;
            schema:name "Charter of Fundamental Rights of the European Union" ;
            schema:url "http://data.europa.eu/eli/treaty/char_2012/oj" ] ;
    rdfs:isDefinedBy eu-rights: ;
    sw:term_status "accepted"@en ;
    skos:broader eu-rights:EUFundamentalRightsImpact ;
    skos:definition "Something that acts as or is considered as an impact on T4 Solidarity"@en ;
    skos:inScheme eu-rights:impacts-classes ;
    skos:prefLabel "Impact on T4 Solidarity"@en .

eu-rights:T5-CitizensRightsImpact a rdfs:Class,
        skos:Concept,
        dpv:RiskConcept,
        risk:PotentialConsequence,
        risk:PotentialImpact,
        risk:PotentialRisk ;
    dct:contributor _:N0a43dd9ea5e94fe695d8b7df8802cfdd ;
    dct:created "2022-08-04"^^xsd:date ;
    dct:source [ a schema:WebPage ;
            schema:name "Charter of Fundamental Rights of the European Union" ;
            schema:url "http://data.europa.eu/eli/treaty/char_2012/oj" ] ;
    rdfs:isDefinedBy eu-rights: ;
    sw:term_status "accepted"@en ;
    skos:broader eu-rights:EUFundamentalRightsImpact ;
    skos:definition "Something that acts as or is considered as an impact on T5 Citizens Rights"@en ;
    skos:inScheme eu-rights:impacts-classes ;
    skos:prefLabel "Impact on T5 Citizens Rights"@en .

eu-rights:T6-JusticeImpact a rdfs:Class,
        skos:Concept,
        dpv:RiskConcept,
        risk:PotentialConsequence,
        risk:PotentialImpact,
        risk:PotentialRisk ;
    dct:contributor _:N0a43dd9ea5e94fe695d8b7df8802cfdd ;
    dct:created "2022-08-13"^^xsd:date ;
    dct:source [ a schema:WebPage ;
            schema:name "Charter of Fundamental Rights of the European Union" ;
            schema:url "http://data.europa.eu/eli/treaty/char_2012/oj" ] ;
    rdfs:isDefinedBy eu-rights: ;
    sw:term_status "accepted"@en ;
    skos:broader eu-rights:EUFundamentalRightsImpact ;
    skos:definition "Something that acts as or is considered as an impact on T6 Justice"@en ;
    skos:inScheme eu-rights:impacts-classes ;
    skos:prefLabel "Impact on T6 Justice"@en .

eu-rights:T7-InterpretationAndApplicationImpact a rdfs:Class,
        skos:Concept,
        dpv:RiskConcept,
        risk:PotentialConsequence,
        risk:PotentialImpact,
        risk:PotentialRisk ;
    dct:contributor _:N0a43dd9ea5e94fe695d8b7df8802cfdd ;
    dct:created "2022-08-18"^^xsd:date ;
    dct:source [ a schema:WebPage ;
            schema:name "Charter of Fundamental Rights of the European Union" ;
            schema:url "http://data.europa.eu/eli/treaty/char_2012/oj" ] ;
    rdfs:isDefinedBy eu-rights: ;
    sw:term_status "accepted"@en ;
    skos:broader eu-rights:EUFundamentalRightsImpact ;
    skos:definition "Something that acts as or is considered as an impact on T7 Interpretation And Application"@en ;
    skos:inScheme eu-rights:impacts-classes ;
    skos:prefLabel "Impact on T7 Interpretation And Application"@en .

<https://w3id.org/dpv/rights/eu> a owl:Ontology,
        profile:Profile ;
    dct:bibliographicCitation "Harshvardhan J. Pandit, Beatriz Esteves, Georg P. Krog, Paul Ryan, Delaram Golpayegani, Julian Flake (2025) Data Privacy Vocabulary (DPV) – Version 2.0. In: Demartini, G., et al. The Semantic Web – ISWC 2024. ISWC 2024. Lecture Notes in Computer Science, vol 15233. Springer, Cham. https://doi.org/10.1007/978-3-031-77847-6_10" ;
    dct:conformsTo "http://www.w3.org/2000/01/rdf-schema",
        "http://www.w3.org/2004/02/skos/core" ;
    dct:contributor _:N0a43dd9ea5e94fe695d8b7df8802cfdd ;
    dct:created "2022-08-15"@en ;
    dct:creator _:N0a43dd9ea5e94fe695d8b7df8802cfdd ;
    dct:description "Extension to the Data Privacy Vocabulary (DPV) providing concepts for representing information associated with EU's Fundamental Rights and Freedoms"@en ;
    dct:identifier "https://w3id.org/dpv/rights/eu" ;
    dct:issued "2022-08-15"@en ;
    dct:license <https://www.w3.org/copyright/document-license-2023/> ;
    dct:modified "2025-03-16"@en ;
    dct:publisher <https://www.w3.org/> ;
    dct:source <https://www.w3.org/groups/cg/dpvcg/> ;
    dct:title "EU Fundamental Rights and Freedoms"@en ;
    bibo:doi "10.5281/zenodo.12505841" ;
    bibo:status "http://purl.org/ontology/bibo/status/published" ;
    vann:preferredNamespacePrefix "eu-rights" ;
    vann:preferredNamespaceUri "https://w3id.org/dpv/rights/eu#" ;
    rdfs:Label "EU-RIGHTS"@en ;
    owl:versionIRI <https://w3id.org/dpv/2.1/rights/eu> ;
    owl:versionInfo "2.1" ;
    profile:hasResource <https://w3id.org/dpv/examples>,
        <https://w3id.org/dpv/guides>,
        <https://w3id.org/dpv/primer>,
        eu-rights:serialisation-html,
        eu-rights:serialisation-jsonld,
        eu-rights:serialisation-n3,
        eu-rights:serialisation-rdf,
        eu-rights:serialisation-ttl ;
    profile:isProfileOf rdfs:,
        skos:,
        <https://w3id.org/dpv> ;
    foaf:logo <https://w3id.org/dpv/media/logo.png> ;
    schema:version "2.1" .

eu-rights:serialisation-html a profile:ResourceDescriptor ;
    dct:conformsTo <https://www.w3.org/TR/html/> ;
    dct:format <https://www.iana.org/assignments/media-types/text/html> ;
    dct:title "EU Fundamental Rights and Freedoms - HTML serialiation" ;
    profile:hasArtifact <https://w3id.org/dpv/rights/eu/eu-rights.html> ;
    profile:hasRole role:specification .

eu-rights:serialisation-jsonld a profile:ResourceDescriptor ;
    dct:conformsTo <https://www.w3.org/TR/json-ld11/> ;
    dct:format <https://www.iana.org/assignments/media-types/application/ld+json> ;
    dct:title "EU Fundamental Rights and Freedoms - JSON-LD serialiation" ;
    profile:hasArtifact <https://w3id.org/dpv/rights/eu/eu-rights.jsonld> ;
    profile:hasRole role:vocabulary .

eu-rights:serialisation-n3 a profile:ResourceDescriptor ;
    dct:conformsTo <https://www.w3.org/TeamSubmission/n3/> ;
    dct:format <https://www.iana.org/assignments/media-types/text/n3> ;
    dct:title "EU Fundamental Rights and Freedoms - N3 serialiation" ;
    profile:hasArtifact <https://w3id.org/dpv/rights/eu/eu-rights.n3> ;
    profile:hasRole role:vocabulary .

eu-rights:serialisation-rdf a profile:ResourceDescriptor ;
    dct:conformsTo rdf: ;
    dct:format <https://www.iana.org/assignments/media-types/application/rdf+xml> ;
    dct:title "EU Fundamental Rights and Freedoms - RDF/XML serialiation" ;
    profile:hasArtifact <https://w3id.org/dpv/rights/eu/eu-rights.rdf> ;
    profile:hasRole role:vocabulary .

eu-rights:serialisation-ttl a profile:ResourceDescriptor ;
    dct:conformsTo <https://www.w3.org/TR/turtle/> ;
    dct:format <https://www.iana.org/assignments/media-types/text/turtle> ;
    dct:title "EU Fundamental Rights and Freedoms - Turtle serialiation" ;
    profile:hasArtifact <https://w3id.org/dpv/rights/eu/eu-rights.ttl> ;
    profile:hasRole role:vocabulary .

<https://w3id.org/dpv/examples> a profile:ResourceDescriptor ;
    dct:conformsTo <https://www.w3.org/TR/html/> ;
    dct:format <https://www.iana.org/assignments/media-types/text/html> ;
    dct:title "Examples for Data Privacy Vocabulary" ;
    profile:hasArtifact <https://w3id.org/dpv/examples> ;
    profile:hasRole role:guidance .

<https://w3id.org/dpv/guides> a profile:ResourceDescriptor ;
    dct:conformsTo <https://www.w3.org/TR/html/> ;
    dct:format <https://www.iana.org/assignments/media-types/text/html> ;
    dct:title "Guides for Data Privacy Vocabulary" ;
    profile:hasArtifact <https://w3id.org/dpv/guides> ;
    profile:hasRole role:guidance .

<https://w3id.org/dpv/primer> a profile:ResourceDescriptor ;
    dct:conformsTo <https://www.w3.org/TR/html/> ;
    dct:format <https://www.iana.org/assignments/media-types/text/html> ;
    dct:title "Primer for Data Privacy Vocabulary" ;
    profile:hasArtifact <https://w3id.org/dpv/primer> ;
    profile:hasRole role:guidance .

eu-rights:impacts-classes a skos:ConceptScheme .

_:N313d89a6c37147bfac1bbb4aa7f6510b a foaf:Organization ;
    foaf:name "ADAPT Centre, Dublin City University" .

_:N0a43dd9ea5e94fe695d8b7df8802cfdd a dct:Agent,
        foaf:Person ;
    scoro:hasORCID "0000-0002-5068-3714" ;
    org:memberOf _:N313d89a6c37147bfac1bbb4aa7f6510b ;
    foaf:homepage "https://harshp.com/" ;
    foaf:name "Harshvardhan J. Pandit" .

