@prefix bibo: <http://purl.org/ontology/bibo/> .
@prefix dct: <http://purl.org/dc/terms/> .
@prefix dpv-owl: <https://w3id.org/dpv/owl#> .
@prefix foaf: <http://xmlns.com/foaf/0.1/> .
@prefix org: <http://www.w3.org/ns/org#> .
@prefix owl: <http://www.w3.org/2002/07/owl#> .
@prefix pd-owl: <https://w3id.org/dpv/pd/owl#> .
@prefix profile: <http://www.w3.org/ns/dx/prof/> .
@prefix rdf: <http://www.w3.org/1999/02/22-rdf-syntax-ns#> .
@prefix rdfs: <http://www.w3.org/2000/01/rdf-schema#> .
@prefix role: <http://www.w3.org/ns/dx/prof/role/> .
@prefix schema: <https://schema.org/> .
@prefix scoro: <http://purl.org/spar/scoro/> .
@prefix sector-health-owl: <https://w3id.org/dpv/sector/health/owl#> .
@prefix skos: <http://www.w3.org/2004/02/skos/core#> .
@prefix sw: <http://www.w3.org/2003/06/sw-vocab-status/ns#> .
@prefix tech-owl: <https://w3id.org/dpv/tech/owl#> .
@prefix vann: <http://purl.org/vocab/vann/> .
@prefix xsd: <http://www.w3.org/2001/XMLSchema#> .

sector-health-owl:AccessManagement a rdfs:Class,
        owl:Class,
        dpv-owl:Purpose ;
    dct:created "2024-12-01"^^xsd:date ;
    rdfs:isDefinedBy sector-health-owl: ;
    rdfs:subClassOf sector-health-owl:HealthcareServiceManagement ;
    sw:term_status "accepted"@en ;
    skos:definition "Purposes associated with managing access to infrastructure, resources, and services as part of healthcare"@en ;
    skos:prefLabel "Access Management"@en .

sector-health-owl:AdministrativeServicesProvision a rdfs:Class,
        owl:Class,
        dpv-owl:Purpose ;
    dct:contributor _:person-beatriz-esteves ;
    dct:created "2025-10-28"^^xsd:date ;
    rdfs:isDefinedBy sector-health-owl: ;
    rdfs:subClassOf sector-health-owl:ServiceProvision ;
    sw:term_status "accepted"@en ;
    skos:definition "Purposes associated with the provision of administrative services related to healthcare"@en ;
    skos:prefLabel "Administrative Services Provision"@en .

sector-health-owl:AppointmentScheduling a rdfs:Class,
        owl:Class,
        dpv-owl:Purpose ;
    dct:created "2024-12-01"^^xsd:date ;
    rdfs:isDefinedBy sector-health-owl: ;
    rdfs:subClassOf sector-health-owl:HealthcareServiceManagement ;
    sw:term_status "accepted"@en ;
    skos:definition "Purposes associated with scheduling appointments for use of healthcare services"@en ;
    skos:prefLabel "Appointment Scheduling"@en .

sector-health-owl:BehaviouralHealthDeterminant a rdfs:Class,
        owl:Class,
        dpv-owl:PersonalData ;
    dct:contributor _:person-beatriz-esteves ;
    dct:created "2026-02-04"^^xsd:date ;
    rdfs:isDefinedBy sector-health-owl: ;
    rdfs:subClassOf pd-owl:Health ;
    sw:term_status "accepted"@en ;
    skos:definition "Information about behavioural data impacting on health"@en ;
    skos:prefLabel "Behavioural Health Determinant"@en .

sector-health-owl:BiobankData a rdfs:Class,
        owl:Class,
        dpv-owl:PersonalData ;
    dct:contributor _:person-beatriz-esteves ;
    dct:created "2026-02-04"^^xsd:date ;
    rdfs:isDefinedBy sector-health-owl: ;
    rdfs:subClassOf pd-owl:MedicalHealth ;
    sw:term_status "accepted"@en ;
    skos:definition "Information about electronic health data from biobanks and associated databases"@en ;
    skos:prefLabel "Biobank Data"@en .

sector-health-owl:ClaimAdminData a rdfs:Class,
        owl:Class,
        dpv-owl:PersonalData ;
    dct:contributor _:person-beatriz-esteves ;
    dct:created "2026-02-04"^^xsd:date ;
    rdfs:isDefinedBy sector-health-owl: ;
    rdfs:subClassOf sector-health-owl:HealthAdminData ;
    sw:term_status "accepted"@en ;
    skos:definition "Information about health-related administrative data on claims"@en ;
    skos:prefLabel "Health-related Administrative Data on Claims"@en .

sector-health-owl:ClinicalInvestigationsData a rdfs:Class,
        owl:Class,
        dpv-owl:PersonalData ;
    dct:contributor _:person-beatriz-esteves ;
    dct:created "2026-02-04"^^xsd:date ;
    rdfs:isDefinedBy sector-health-owl: ;
    rdfs:subClassOf sector-health-owl:StudyData ;
    sw:term_status "accepted"@en ;
    skos:definition "Information about health data from clinical investigations"@en ;
    skos:prefLabel "Clinical Investigations Data"@en .

sector-health-owl:ClinicalStudiesData a rdfs:Class,
        owl:Class,
        dpv-owl:PersonalData ;
    dct:contributor _:person-beatriz-esteves ;
    dct:created "2026-02-04"^^xsd:date ;
    rdfs:isDefinedBy sector-health-owl: ;
    rdfs:subClassOf sector-health-owl:StudyData ;
    sw:term_status "accepted"@en ;
    skos:definition "Information about health data from clinical studies"@en ;
    skos:prefLabel "Clinical Studies Data"@en .

sector-health-owl:ClinicalTrialsData a rdfs:Class,
        owl:Class,
        dpv-owl:PersonalData ;
    dct:contributor _:person-beatriz-esteves ;
    dct:created "2026-02-04"^^xsd:date ;
    rdfs:isDefinedBy sector-health-owl: ;
    rdfs:subClassOf sector-health-owl:StudyData ;
    sw:term_status "accepted"@en ;
    skos:definition "Information about health data from clinical trials"@en ;
    skos:prefLabel "Clinical Trials Data"@en .

sector-health-owl:CompatibilityUnknown a rdfs:Class,
        owl:Class,
        sector-health-owl:ReuseCompatibility ;
    dct:contributor _:person-arthit-suriyawongkul,
        _:person-beatriz-esteves,
        _:person-delaram-golpayegani,
        _:person-georg-p-krog,
        _:person-harshvardhan-j-pandit,
        _:person-julian-flake ;
    dct:created "2025-06-19"^^xsd:date ;
    rdfs:isDefinedBy sector-health-owl: ;
    rdfs:subClassOf dpv-owl:CompatibilityUnknown ;
    sw:term_status "accepted"@en ;
    skos:definition "Status indicating the compatibility for reuse of health data for the context is currently unknown"@en ;
    skos:prefLabel "Compatibility Unknown"@en .

sector-health-owl:ConsultationManagement a rdfs:Class,
        owl:Class,
        dpv-owl:Purpose ;
    dct:created "2024-12-01"^^xsd:date ;
    rdfs:isDefinedBy sector-health-owl: ;
    rdfs:subClassOf sector-health-owl:ServiceProvision ;
    sw:term_status "accepted"@en ;
    skos:definition "Purposes associated with managing consultations as part of healthcare services"@en ;
    skos:prefLabel "Consultation Management"@en .

sector-health-owl:CrisisManagement a rdfs:Class,
        owl:Class,
        dpv-owl:Purpose ;
    dct:created "2024-12-01"^^xsd:date ;
    rdfs:isDefinedBy sector-health-owl: ;
    rdfs:subClassOf dpv-owl:ImproveHealthcare,
        sector-health-owl:HealthcareServiceManagement ;
    sw:term_status "accepted"@en ;
    skos:definition "Purposes associated with management of crisis situations in relation to healthcare services"@en ;
    skos:prefLabel "Crisis Management"@en .

sector-health-owl:DevelopPublicHealthProductsAndServices a rdfs:Class,
        owl:Class,
        dpv-owl:Purpose ;
    dct:contributor _:person-beatriz-esteves ;
    dct:created "2026-02-04"^^xsd:date ;
    rdfs:isDefinedBy sector-health-owl: ;
    rdfs:subClassOf dpv-owl:ResearchAndDevelopment ;
    sw:term_status "accepted"@en ;
    skos:definition "Purposes associated with developing products and services that contribute to public health"@en ;
    skos:prefLabel "Develop Public Health Products and Services"@en .

sector-health-owl:DevelopSocialSecurityProductsAndServices a rdfs:Class,
        owl:Class,
        dpv-owl:Purpose ;
    dct:contributor _:person-beatriz-esteves ;
    dct:created "2026-02-04"^^xsd:date ;
    rdfs:isDefinedBy sector-health-owl: ;
    rdfs:subClassOf dpv-owl:ResearchAndDevelopment ;
    sw:term_status "accepted"@en ;
    skos:definition "Purposes associated with developing products and services that contribute to social security"@en ;
    skos:prefLabel "Develop Social Security Products and Services"@en .

sector-health-owl:DiagnosisManagement a rdfs:Class,
        owl:Class,
        dpv-owl:Purpose ;
    dct:created "2024-12-01"^^xsd:date ;
    rdfs:isDefinedBy sector-health-owl: ;
    rdfs:subClassOf sector-health-owl:ServiceProvision ;
    sw:term_status "accepted"@en ;
    skos:definition "Purposes associated with conducting and managing diagnosis as part of healthcare services"@en ;
    skos:prefLabel "Diagnosis Management"@en .

sector-health-owl:DiagnosticOptimisation a rdfs:Class,
        owl:Class,
        dpv-owl:Purpose ;
    dct:created "2024-12-01"^^xsd:date ;
    rdfs:isDefinedBy sector-health-owl: ;
    rdfs:subClassOf dpv-owl:ServiceOptimisation,
        sector-health-owl:Optimisation ;
    sw:term_status "accepted"@en ;
    skos:definition "Purposes associated with identifying optimisations related to use of diagnosis tools and processes as part of healthcare services"@en ;
    skos:prefLabel "Diagnostic Optimisation"@en .

sector-health-owl:DigitalHealthAuthority a rdfs:Class,
        owl:Class,
        dpv-owl:LegalEntity ;
    dct:contributor _:person-beatriz-esteves ;
    dct:created "2026-02-04"^^xsd:date ;
    dct:source "EHDS Art.19"@en ;
    rdfs:isDefinedBy sector-health-owl: ;
    rdfs:subClassOf dpv-owl:Authority ;
    sw:term_status "accepted"@en ;
    skos:definition "An authority tasked with overseeing the implementation and enforcement of primary use provisions"@en ;
    skos:prefLabel "Digital Health Authority"@en .

sector-health-owl:DisasterReliefManagement a rdfs:Class,
        owl:Class,
        dpv-owl:Purpose ;
    dct:created "2024-12-01"^^xsd:date ;
    rdfs:isDefinedBy sector-health-owl: ;
    rdfs:subClassOf sector-health-owl:CrisisManagement ;
    sw:term_status "accepted"@en ;
    skos:definition "Purposes associated with management of disaster relief and related crisis situations in relation to healthcare services"@en ;
    skos:prefLabel "Disaster Relief Management"@en .

sector-health-owl:DischargeReport a rdfs:Class,
        owl:Class,
        dpv-owl:PersonalData ;
    dct:contributor _:person-beatriz-esteves ;
    dct:created "2025-10-28"^^xsd:date ;
    rdfs:isDefinedBy sector-health-owl: ;
    rdfs:subClassOf pd-owl:HealthRecord ;
    sw:term_status "accepted"@en ;
    skos:definition "Information about discharge reports"@en ;
    skos:prefLabel "Discharge Report"@en .

sector-health-owl:DiseasePreventionAwareness a rdfs:Class,
        owl:Class,
        dpv-owl:Purpose ;
    dct:created "2024-12-01"^^xsd:date ;
    rdfs:isDefinedBy sector-health-owl: ;
    rdfs:subClassOf sector-health-owl:PreventativeCareManagement ;
    sw:term_status "accepted"@en ;
    skos:definition "Purposes associated with management of disease prevention awareness as part of healthcare services"@en ;
    skos:prefLabel "Disease Prevention Awareness"@en .

sector-health-owl:DiseaseRegistryData a rdfs:Class,
        owl:Class,
        dpv-owl:PersonalData ;
    dct:contributor _:person-beatriz-esteves ;
    dct:created "2026-02-04"^^xsd:date ;
    rdfs:isDefinedBy sector-health-owl: ;
    rdfs:subClassOf sector-health-owl:MedicalRegistryData ;
    sw:term_status "accepted"@en ;
    skos:definition "Information about electronic health data from medical registries for specific diseases"@en ;
    skos:prefLabel "Disease Registry Data"@en .

sector-health-owl:DispensationAdminData a rdfs:Class,
        owl:Class,
        dpv-owl:PersonalData ;
    dct:contributor _:person-beatriz-esteves ;
    dct:created "2026-02-04"^^xsd:date ;
    rdfs:isDefinedBy sector-health-owl: ;
    rdfs:subClassOf sector-health-owl:HealthAdminData ;
    sw:term_status "accepted"@en ;
    skos:definition "Information about health-related administrative data on dispensations"@en ;
    skos:prefLabel "Health-related Administrative Data on Dispensations"@en .

sector-health-owl:DispensationManagement a rdfs:Class,
        owl:Class,
        dpv-owl:Purpose ;
    dct:contributor _:person-beatriz-esteves ;
    dct:created "2025-10-28"^^xsd:date ;
    rdfs:isDefinedBy sector-health-owl: ;
    rdfs:subClassOf sector-health-owl:ServiceProvision ;
    sw:term_status "accepted"@en ;
    skos:definition "Purposes associated with dispensation of products, devices and other healthcare-related resources"@en ;
    skos:prefLabel "Dispensation Management"@en .

sector-health-owl:EHRData a rdfs:Class,
        owl:Class,
        dpv-owl:PersonalData ;
    dct:contributor _:person-beatriz-esteves ;
    dct:created "2026-02-04"^^xsd:date ;
    rdfs:isDefinedBy sector-health-owl: ;
    rdfs:subClassOf pd-owl:HealthRecord ;
    sw:term_status "accepted"@en ;
    skos:definition "Information about electronic health record data"@en ;
    skos:prefLabel "Electronic Health Record (EHR) Data"@en .

sector-health-owl:EHRSystem a rdfs:Class,
        owl:Class,
        dpv-owl:Technology ;
    dct:contributor _:person-beatriz-esteves ;
    dct:created "2025-10-28"^^xsd:date ;
    rdfs:isDefinedBy sector-health-owl: ;
    rdfs:subClassOf sector-health-owl:System ;
    sw:term_status "accepted"@en ;
    skos:definition "A system whereby the software and/or hardware allows electronic health record data to be collected and processed, to be used by healthcare providers when providing patient care or by patients when accessing their electronic health data"@en ;
    skos:prefLabel "Electronic Health Record System"@en .

sector-health-owl:EHRSystemDistributor a rdfs:Class,
        owl:Class,
        tech-owl:Actor ;
    dct:contributor _:person-beatriz-esteves ;
    dct:created "2026-02-04"^^xsd:date ;
    dct:source "EHDS Art.33"@en ;
    rdfs:isDefinedBy sector-health-owl: ;
    rdfs:subClassOf tech-owl:Distributor ;
    sw:term_status "accepted"@en ;
    skos:definition "Actor that distributes electronic health record systems"@en ;
    skos:prefLabel "Electronic Health Record System Distributor"@en .

sector-health-owl:EHRSystemImporter a rdfs:Class,
        owl:Class,
        tech-owl:Actor ;
    dct:contributor _:person-beatriz-esteves ;
    dct:created "2026-02-04"^^xsd:date ;
    dct:source "EHDS Art.32"@en ;
    rdfs:isDefinedBy sector-health-owl: ;
    rdfs:subClassOf tech-owl:Importer ;
    sw:term_status "accepted"@en ;
    skos:definition "Actor that imports electronic health record systems"@en ;
    skos:prefLabel "Electronic Health Record System Importer"@en .

sector-health-owl:EHRSystemManufacturer a rdfs:Class,
        owl:Class,
        tech-owl:Actor ;
    dct:contributor _:person-beatriz-esteves ;
    dct:created "2026-02-04"^^xsd:date ;
    rdfs:isDefinedBy sector-health-owl: ;
    rdfs:subClassOf tech-owl:Manufacturer ;
    sw:term_status "accepted"@en ;
    skos:definition "Actor that manufactures electronic health record systems"@en ;
    skos:prefLabel "Electronic Health Record System Manufacturer"@en .

sector-health-owl:EHRSystemSupplier a rdfs:Class,
        owl:Class,
        tech-owl:Actor ;
    dct:contributor _:person-beatriz-esteves ;
    dct:created "2026-02-04"^^xsd:date ;
    rdfs:isDefinedBy sector-health-owl: ;
    rdfs:subClassOf tech-owl:Supplier ;
    sw:term_status "accepted"@en ;
    skos:definition "Actor that supplies electronic health record systems"@en ;
    skos:prefLabel "Electronic Health Record System Supplier"@en .

sector-health-owl:EffectivenessAssessment a rdfs:Class,
        owl:Class,
        dpv-owl:Purpose ;
    dct:created "2024-12-01"^^xsd:date ;
    rdfs:isDefinedBy sector-health-owl: ;
    rdfs:subClassOf sector-health-owl:ResearchDevelopment ;
    sw:term_status "accepted"@en ;
    skos:definition "Purposes associated with assessing the effectiveness of healthcare infrastructure and services"@en ;
    skos:prefLabel "Effectiveness Assessment"@en .

sector-health-owl:ElectronicDispensation a rdfs:Class,
        owl:Class,
        dpv-owl:PersonalData ;
    dct:contributor _:person-beatriz-esteves ;
    dct:created "2025-10-28"^^xsd:date ;
    rdfs:isDefinedBy sector-health-owl: ;
    rdfs:subClassOf pd-owl:HealthRecord ;
    sw:term_status "accepted"@en ;
    skos:definition "Information about electronic dispensations"@en ;
    skos:prefLabel "Electronic Dispensation"@en .

sector-health-owl:ElectronicHealthData a rdfs:Class,
        owl:Class,
        dpv-owl:PersonalData ;
    dct:contributor _:person-beatriz-esteves ;
    dct:created "2025-10-28"^^xsd:date ;
    rdfs:isDefinedBy sector-health-owl: ;
    rdfs:subClassOf dpv-owl:PersonalData ;
    sw:term_status "accepted"@en ;
    skos:definition "Information about electronic health data, including personal and non-personal data"@en ;
    skos:prefLabel "Electronic Health Data"@en .

sector-health-owl:ElectronicHealthDataAccessService a rdfs:Class,
        owl:Class,
        dpv-owl:Technology ;
    dct:contributor _:person-beatriz-esteves ;
    dct:created "2025-10-28"^^xsd:date ;
    rdfs:isDefinedBy sector-health-owl: ;
    rdfs:subClassOf tech-owl:Service ;
    sw:term_status "accepted"@en ;
    skos:definition "Technical service, such as an online portal or application, that allows data subjects to access their electronic health data or the electronic health data of those natural persons whose electronic health data they are legally authorised to access"@en ;
    skos:prefLabel "Electronic Health Data Access Service"@en .

sector-health-owl:ElectronicPrescription a rdfs:Class,
        owl:Class,
        dpv-owl:PersonalData ;
    dct:contributor _:person-beatriz-esteves ;
    dct:created "2025-10-28"^^xsd:date ;
    rdfs:isDefinedBy sector-health-owl: ;
    rdfs:subClassOf pd-owl:HealthRecord ;
    sw:term_status "accepted"@en ;
    skos:definition "Information about electronic prescriptions"@en ;
    skos:prefLabel "Electronic Prescription"@en .

sector-health-owl:ElectronicRecordsManagement a rdfs:Class,
        owl:Class,
        dpv-owl:Purpose ;
    dct:created "2024-12-01"^^xsd:date ;
    rdfs:isDefinedBy sector-health-owl: ;
    rdfs:subClassOf sector-health-owl:PatientInformationManagement ;
    sw:term_status "accepted"@en ;
    skos:definition "Purposes associated with management of patient information in electronic forms for healthcare services"@en ;
    skos:prefLabel "Electronic Records Management"@en .

sector-health-owl:EligibilityAssessment a rdfs:Class,
        owl:Class,
        dpv-owl:Purpose ;
    dct:created "2024-12-01"^^xsd:date ;
    rdfs:isDefinedBy sector-health-owl: ;
    rdfs:subClassOf sector-health-owl:HealthcareServiceManagement ;
    sw:term_status "accepted"@en ;
    skos:definition "Purposes associated with assessment of eligibility to receive or continue to receive healthcare services"@en ;
    skos:prefLabel "Eligibility Assessment"@en .

sector-health-owl:EmergencyCareCommunication a rdfs:Class,
        owl:Class,
        dpv-owl:Purpose ;
    dct:created "2024-12-01"^^xsd:date ;
    rdfs:isDefinedBy sector-health-owl: ;
    rdfs:subClassOf sector-health-owl:EmergencyCareManagement ;
    sw:term_status "accepted"@en ;
    skos:definition "Purposes associated with management of communication for emergency care as part of healthcare services"@en ;
    skos:prefLabel "Emergency Care Communication"@en .

sector-health-owl:EmergencyCareDispatch a rdfs:Class,
        owl:Class,
        dpv-owl:Purpose ;
    dct:created "2024-12-01"^^xsd:date ;
    rdfs:isDefinedBy sector-health-owl: ;
    rdfs:subClassOf sector-health-owl:EmergencyCareManagement ;
    sw:term_status "accepted"@en ;
    skos:definition "Purposes associated with management of emergency care dispatch as part of healthcare services"@en ;
    skos:prefLabel "Emergency Care Dispatch"@en .

sector-health-owl:EmergencyCareEligibilityAssessment a rdfs:Class,
        owl:Class,
        dpv-owl:Purpose ;
    dct:created "2024-12-01"^^xsd:date ;
    rdfs:isDefinedBy sector-health-owl: ;
    rdfs:subClassOf sector-health-owl:EmergencyCareManagement ;
    sw:term_status "accepted"@en ;
    skos:definition "Purposes associated with assessment of eligibility to receive or continue to receive emergency care as part of healthcare services"@en ;
    skos:prefLabel "Emergency Care Eligibility Assessment"@en .

sector-health-owl:EmergencyCareManagement a rdfs:Class,
        owl:Class,
        dpv-owl:Purpose ;
    dct:created "2024-12-01"^^xsd:date ;
    rdfs:isDefinedBy sector-health-owl: ;
    rdfs:subClassOf sector-health-owl:HealthcareServiceManagement ;
    sw:term_status "accepted"@en ;
    skos:definition "Purposes associated with management of emergency care as part of healthcare services"@en ;
    skos:prefLabel "Emergency Care Management"@en .

sector-health-owl:EmergencyCareTriage a rdfs:Class,
        owl:Class,
        dpv-owl:Purpose ;
    dct:created "2024-12-01"^^xsd:date ;
    rdfs:isDefinedBy sector-health-owl: ;
    rdfs:subClassOf sector-health-owl:EmergencyCareManagement ;
    sw:term_status "accepted"@en ;
    skos:definition "Purposes associated with management of prioritisation and other triage processes as part of emergency care in healthcare services"@en ;
    skos:prefLabel "Emergency Care Triage"@en .

sector-health-owl:EnsureQualitySafetyHealthcare a rdfs:Class,
        owl:Class,
        dpv-owl:Purpose ;
    dct:contributor _:person-beatriz-esteves ;
    dct:created "2026-02-04"^^xsd:date ;
    rdfs:isDefinedBy sector-health-owl: ;
    rdfs:subClassOf sector-health-owl:PublicInterestRelatedToHealth ;
    sw:term_status "accepted"@en ;
    skos:definition "Purposes associated with ensuring high levels of quality and safety of healthcare, including patients safety"@en ;
    skos:prefLabel "Ensure Quality and Safety of Healthcare"@en .

sector-health-owl:EnsureQualitySafetyMedicalDevices a rdfs:Class,
        owl:Class,
        dpv-owl:Purpose ;
    dct:contributor _:person-beatriz-esteves ;
    dct:created "2026-02-04"^^xsd:date ;
    rdfs:isDefinedBy sector-health-owl: ;
    rdfs:subClassOf sector-health-owl:PublicInterestRelatedToHealth ;
    sw:term_status "accepted"@en ;
    skos:definition "Purposes associated with ensuring high levels of quality and safety of medical devices"@en ;
    skos:prefLabel "Ensure Quality and Safety of Medical Devices"@en .

sector-health-owl:EnsureQualitySafetyMedicinalProducts a rdfs:Class,
        owl:Class,
        dpv-owl:Purpose ;
    dct:contributor _:person-beatriz-esteves ;
    dct:created "2026-02-04"^^xsd:date ;
    rdfs:isDefinedBy sector-health-owl: ;
    rdfs:subClassOf sector-health-owl:PublicInterestRelatedToHealth ;
    sw:term_status "accepted"@en ;
    skos:definition "Purposes associated with ensuring high levels of quality and safety of medicinal products"@en ;
    skos:prefLabel "Ensure Quality and Safety of Medicinal Products"@en .

sector-health-owl:EnvironmentalHealthDeterminant a rdfs:Class,
        owl:Class,
        dpv-owl:PersonalData ;
    dct:contributor _:person-beatriz-esteves ;
    dct:created "2026-02-04"^^xsd:date ;
    rdfs:isDefinedBy sector-health-owl: ;
    rdfs:subClassOf pd-owl:Health ;
    sw:term_status "accepted"@en ;
    skos:definition "Information about environmental data impacting on health"@en ;
    skos:prefLabel "Environmental Health Determinant"@en .

sector-health-owl:EpigenomicData a rdfs:Class,
        owl:Class,
        dpv-owl:PersonalData ;
    dct:contributor _:person-beatriz-esteves ;
    dct:created "2026-02-04"^^xsd:date ;
    rdfs:isDefinedBy sector-health-owl: ;
    rdfs:subClassOf pd-owl:Genetic ;
    sw:term_status "accepted"@en ;
    skos:definition "Information about epigenomic data"@en ;
    skos:prefLabel "Epigenomic Data"@en .

sector-health-owl:FitnessNutritionAwareness a rdfs:Class,
        owl:Class,
        dpv-owl:Purpose ;
    dct:created "2024-12-01"^^xsd:date ;
    rdfs:isDefinedBy sector-health-owl: ;
    rdfs:subClassOf sector-health-owl:PreventativeCareManagement ;
    sw:term_status "accepted"@en ;
    skos:definition "Purposes associated with management of fitness and nutrition awareness as part of healthcare services"@en ;
    skos:prefLabel "Fitness Nutrition Awareness"@en .

sector-health-owl:FraudPreventionDetection a rdfs:Class,
        owl:Class,
        dpv-owl:Purpose ;
    dct:created "2024-12-01"^^xsd:date ;
    rdfs:isDefinedBy sector-health-owl: ;
    rdfs:subClassOf dpv-owl:FraudPreventionAndDetection,
        sector-health-owl:SecurityManagement ;
    sw:term_status "accepted"@en ;
    skos:definition "Purposes associated with fraud prevention and detection in relation to healthcare services"@en ;
    skos:prefLabel "Fraud Prevention Detection"@en .

sector-health-owl:GeneticConditionDiagnosis a rdfs:Class,
        owl:Class,
        dpv-owl:Purpose ;
    dct:created "2024-12-01"^^xsd:date ;
    rdfs:isDefinedBy sector-health-owl: ;
    rdfs:subClassOf sector-health-owl:DiagnosisManagement ;
    sw:term_status "accepted"@en ;
    skos:definition "Purposes associated with conducting and managing genetic diagnosis as part of healthcare services"@en ;
    skos:prefLabel "Genetic Condition Diagnosis"@en .

sector-health-owl:GenomicData a rdfs:Class,
        owl:Class,
        dpv-owl:PersonalData ;
    dct:contributor _:person-beatriz-esteves ;
    dct:created "2026-02-04"^^xsd:date ;
    rdfs:isDefinedBy sector-health-owl: ;
    rdfs:subClassOf pd-owl:Genetic ;
    sw:term_status "accepted"@en ;
    skos:definition "Information about genomic data"@en ;
    skos:prefLabel "Genomic Data"@en .

sector-health-owl:HealthAdminData a rdfs:Class,
        owl:Class,
        dpv-owl:PersonalData ;
    dct:contributor _:person-beatriz-esteves ;
    dct:created "2026-02-04"^^xsd:date ;
    rdfs:isDefinedBy sector-health-owl: ;
    rdfs:subClassOf pd-owl:MedicalHealth ;
    sw:term_status "accepted"@en ;
    skos:definition "Information about health-related administrative data"@en ;
    skos:prefLabel "Health-related Administrative Data"@en .

sector-health-owl:HealthAggregatedData a rdfs:Class,
        owl:Class,
        dpv-owl:AggregatedData ;
    dct:contributor _:person-beatriz-esteves ;
    dct:created "2026-02-04"^^xsd:date ;
    rdfs:isDefinedBy sector-health-owl: ;
    rdfs:subClassOf pd-owl:Health ;
    sw:term_status "accepted"@en ;
    skos:definition "Information about aggregated data related to health and healthcare"@en ;
    skos:prefLabel "Health Aggregated Data"@en .

sector-health-owl:HealthApplication a rdfs:Class,
        owl:Class,
        dpv-owl:Technology ;
    dct:contributor _:person-beatriz-esteves ;
    dct:created "2025-10-28"^^xsd:date ;
    rdfs:isDefinedBy sector-health-owl: ;
    rdfs:subClassOf tech-owl:Application ;
    sw:term_status "accepted"@en ;
    skos:definition "Software component for the processing of electronic health data, specifically for providing information on the health of natural persons, or the delivery of care for purposes other than the provision of healthcare"@en ;
    skos:prefLabel "Health Application"@en .

sector-health-owl:HealthDataAccessBody a rdfs:Class,
        owl:Class ;
    dct:contributor _:person-beatriz-esteves ;
    dct:created "2026-02-04"^^xsd:date ;
    rdfs:isDefinedBy sector-health-owl: ;
    sw:term_status "accepted"@en ;
    skos:definition "An entity responsible for granting access to electronic health data for secondary use"@en ;
    skos:prefLabel "Health Data Access Body"@en .

sector-health-owl:HealthDataHolder a rdfs:Class,
        owl:Class ;
    dct:contributor _:person-julian-flake ;
    dct:created "2026-02-06"^^xsd:date ;
    rdfs:isDefinedBy sector-health-owl: ;
    rdfs:subClassOf dpv-owl:Entity ;
    sw:term_status "accepted"@en ;
    skos:definition "Entity that has the authority to use and make available health data (draft definition)"@en ;
    skos:prefLabel "Health Data Holder"@en .

sector-health-owl:HealthDataUser a rdfs:Class,
        owl:Class ;
    dct:contributor _:person-julian-flake ;
    dct:created "2026-02-06"^^xsd:date ;
    rdfs:isDefinedBy sector-health-owl: ;
    rdfs:subClassOf dpv-owl:Entity ;
    sw:term_status "accepted"@en ;
    skos:definition "Entity that has requested or obtained access to use health data (draft definition)"@en ;
    skos:prefLabel "Health Data User"@en .

sector-health-owl:HealthInequalityAnalysis a rdfs:Class,
        owl:Class,
        dpv-owl:Purpose ;
    dct:created "2024-12-01"^^xsd:date ;
    rdfs:isDefinedBy sector-health-owl: ;
    rdfs:subClassOf sector-health-owl:ResearchDevelopment ;
    sw:term_status "accepted"@en ;
    skos:definition "Purposes associated with detecting, analysing, and identifying ways to mitigate inequality in provision and use of healthcare services"@en ;
    skos:prefLabel "Health Inequality Analysis"@en .

sector-health-owl:HealthInsuranceManagement a rdfs:Class,
        owl:Class,
        dpv-owl:Purpose ;
    dct:created "2024-12-01"^^xsd:date ;
    rdfs:isDefinedBy sector-health-owl: ;
    rdfs:subClassOf sector-health-owl:InsuranceManagement ;
    sw:term_status "accepted"@en ;
    skos:definition "Purposes associated with managing health insurance as part of healthcare services"@en ;
    skos:prefLabel "Health Insurance Management"@en .

sector-health-owl:HealthProfessional a rdfs:Class,
        owl:Class ;
    dct:contributor _:person-beatriz-esteves ;
    dct:created "2026-02-04"^^xsd:date ;
    rdfs:isDefinedBy sector-health-owl: ;
    sw:term_status "accepted"@en ;
    skos:definition "An entity that works as a health professional"@en ;
    skos:prefLabel "Health Professional"@en .

sector-health-owl:HealthProfessionalAccessService a rdfs:Class,
        owl:Class,
        dpv-owl:Technology ;
    dct:contributor _:person-beatriz-esteves ;
    dct:created "2025-10-28"^^xsd:date ;
    rdfs:isDefinedBy sector-health-owl: ;
    rdfs:subClassOf tech-owl:Service ;
    sw:term_status "accepted"@en ;
    skos:definition "Technical service, supported by an EHR system, that enables health professionals to access data of natural persons under their care"@en ;
    skos:prefLabel "Health Professional Access Service"@en .

sector-health-owl:HealthProfessionalData a rdfs:Class,
        owl:Class,
        dpv-owl:PersonalData ;
    dct:contributor _:person-beatriz-esteves ;
    dct:created "2026-02-04"^^xsd:date ;
    rdfs:isDefinedBy sector-health-owl: ;
    rdfs:subClassOf pd-owl:HealthRecord ;
    sw:term_status "accepted"@en ;
    skos:definition "Information about the status of the health professionals involved in the treatment of the person, including information on their specialisation and institution"@en ;
    skos:prefLabel "Health Professional Data"@en .

sector-health-owl:HealthQuestionnaire a rdfs:Class,
        owl:Class,
        dpv-owl:PersonalData ;
    dct:contributor _:person-beatriz-esteves ;
    dct:created "2026-02-04"^^xsd:date ;
    rdfs:isDefinedBy sector-health-owl: ;
    rdfs:subClassOf sector-health-owl:StudyData ;
    sw:term_status "accepted"@en ;
    skos:definition "Information about health data from questionnaires"@en ;
    skos:prefLabel "Health Questionnaire"@en .

sector-health-owl:HealthRegistryData a rdfs:Class,
        owl:Class,
        dpv-owl:PersonalData ;
    dct:contributor _:person-beatriz-esteves ;
    dct:created "2026-02-04"^^xsd:date ;
    rdfs:isDefinedBy sector-health-owl: ;
    rdfs:subClassOf pd-owl:MedicalHealth ;
    sw:term_status "accepted"@en ;
    skos:definition "Information about registries of health data"@en ;
    skos:prefLabel "Health Registry Data"@en .

sector-health-owl:HealthSurvey a rdfs:Class,
        owl:Class,
        dpv-owl:PersonalData ;
    dct:contributor _:person-beatriz-esteves ;
    dct:created "2026-02-04"^^xsd:date ;
    rdfs:isDefinedBy sector-health-owl: ;
    rdfs:subClassOf sector-health-owl:StudyData ;
    sw:term_status "accepted"@en ;
    skos:definition "Information about health data from surveys"@en ;
    skos:prefLabel "Health Survey"@en .

sector-health-owl:HealthTrendAnalysis a rdfs:Class,
        owl:Class,
        dpv-owl:Purpose ;
    dct:created "2024-12-01"^^xsd:date ;
    rdfs:isDefinedBy sector-health-owl: ;
    rdfs:subClassOf sector-health-owl:ResearchDevelopment ;
    sw:term_status "accepted"@en ;
    skos:definition "Purposes associated with analysing trends in public health and safety"@en ;
    skos:prefLabel "Health Trend Analysis"@en .

sector-health-owl:HealthcareManagement a rdfs:Class,
        owl:Class,
        dpv-owl:Purpose ;
    dct:created "2024-12-01"^^xsd:date ;
    rdfs:isDefinedBy sector-health-owl: ;
    rdfs:subClassOf dpv-owl:Purpose ;
    sw:term_status "accepted"@en ;
    skos:definition "Purposes associated with management of healthcare infrastructure and services"@en ;
    skos:prefLabel "Healthcare Management"@en .

sector-health-owl:HealthcareProvider a rdfs:Class,
        owl:Class ;
    dct:contributor _:person-beatriz-esteves ;
    dct:created "2026-02-04"^^xsd:date ;
    rdfs:isDefinedBy sector-health-owl: ;
    sw:term_status "accepted"@en ;
    skos:definition "An entity that provides healthcare-related services"@en ;
    skos:prefLabel "Healthcare Provider"@en .

sector-health-owl:HealthcareScientificResearch a rdfs:Class,
        owl:Class,
        dpv-owl:Purpose ;
    dct:contributor _:person-beatriz-esteves ;
    dct:created "2026-02-04"^^xsd:date ;
    rdfs:isDefinedBy sector-health-owl: ;
    rdfs:subClassOf dpv-owl:ScientificResearch ;
    sw:term_status "accepted"@en ;
    skos:definition "Purposes associated with healthcare scientific research"@en ;
    skos:prefLabel "Healthcare Scientific Research"@en .

sector-health-owl:HealthcareServiceManagement a rdfs:Class,
        owl:Class,
        dpv-owl:Purpose ;
    dct:created "2024-12-01"^^xsd:date ;
    rdfs:isDefinedBy sector-health-owl: ;
    rdfs:subClassOf sector-health-owl:HealthcareManagement ;
    sw:term_status "accepted"@en ;
    skos:definition "Purposes associated with management of healthcare services"@en ;
    skos:prefLabel "Healthcare Service Management"@en .

sector-health-owl:HomeCareManagement a rdfs:Class,
        owl:Class,
        dpv-owl:Purpose ;
    dct:contributor _:person-beatriz-esteves ;
    dct:created "2025-10-28"^^xsd:date ;
    rdfs:isDefinedBy sector-health-owl: ;
    rdfs:subClassOf sector-health-owl:PrimaryCareManagement ;
    sw:term_status "accepted"@en ;
    skos:definition "Purposes associated with management of home healthcare services"@en ;
    skos:prefLabel "Home Care Management"@en .

sector-health-owl:IdentityFraudManagement a rdfs:Class,
        owl:Class,
        dpv-owl:Purpose ;
    dct:created "2024-12-01"^^xsd:date ;
    rdfs:isDefinedBy sector-health-owl: ;
    rdfs:subClassOf sector-health-owl:FraudPreventionDetection ;
    sw:term_status "accepted"@en ;
    skos:definition "Purposes associated with identity prevention and detection in relation to healthcare services"@en ;
    skos:prefLabel "Identity Fraud Management"@en .

sector-health-owl:ImproveHealthcare a rdfs:Class,
        owl:Class,
        dpv-owl:Purpose ;
    dct:contributor _:person-beatriz-esteves ;
    dct:created "2026-02-04"^^xsd:date ;
    rdfs:isDefinedBy sector-health-owl: ;
    rdfs:subClassOf dpv-owl:ImproveHealthcare ;
    sw:term_status "accepted"@en ;
    skos:definition "Purposes associated with improving healthcare systems, including the delivery of care and the provision and optimisation of treatment"@en ;
    skos:prefLabel "Improve Healthcare"@en .

sector-health-owl:ImproveHealthcareEducation a rdfs:Class,
        owl:Class,
        dpv-owl:Purpose ;
    dct:contributor _:person-beatriz-esteves ;
    dct:created "2026-02-04"^^xsd:date ;
    rdfs:isDefinedBy sector-health-owl: ;
    rdfs:subClassOf dpv-owl:ImprovePublicServices ;
    sw:term_status "accepted"@en ;
    skos:definition "Purposes associated with improving the provision of healthcare education"@en ;
    skos:prefLabel "Improve Healthcare Education"@en .

sector-health-owl:InferredHealthData a rdfs:Class,
        owl:Class,
        dpv-owl:PersonalData ;
    dct:contributor _:person-beatriz-esteves ;
    dct:created "2026-02-04"^^xsd:date ;
    rdfs:isDefinedBy sector-health-owl: ;
    rdfs:subClassOf dpv-owl:InferredPersonalData ;
    sw:term_status "accepted"@en ;
    skos:definition "Information about inferred health data, including improvements such as correction, annotation, or enrichment based on authorised processing operations"@en ;
    skos:prefLabel "Inferred Health Data"@en .

sector-health-owl:InsuranceClaimFraudManagement a rdfs:Class,
        owl:Class,
        dpv-owl:Purpose ;
    dct:created "2024-12-01"^^xsd:date ;
    rdfs:isDefinedBy sector-health-owl: ;
    rdfs:subClassOf sector-health-owl:FraudPreventionDetection ;
    sw:term_status "accepted"@en ;
    skos:definition "Purposes associated with insurance fraud prevention and detection in relation to healthcare services"@en ;
    skos:prefLabel "Insurance Claim Fraud Management"@en .

sector-health-owl:InsuranceManagement a rdfs:Class,
        owl:Class,
        dpv-owl:Purpose ;
    dct:created "2024-12-01"^^xsd:date ;
    dct:modified "2025-10-28"^^xsd:date ;
    rdfs:isDefinedBy sector-health-owl: ;
    rdfs:subClassOf dpv-owl:InsuranceManagement,
        sector-health-owl:HealthcareManagement ;
    sw:term_status "modified"@en ;
    skos:definition "Purposes associated with management of insurance as part of providing healthcare services"@en ;
    skos:prefLabel "Insurance Management"@en .

sector-health-owl:InteroperabilitySoftwareForEHRSystem a rdfs:Class,
        owl:Class,
        dpv-owl:Technology ;
    dct:contributor _:person-beatriz-esteves ;
    dct:created "2025-10-28"^^xsd:date ;
    rdfs:isDefinedBy sector-health-owl: ;
    rdfs:subClassOf tech-owl:Software ;
    sw:term_status "accepted"@en ;
    skos:definition "Software component of the EHR system which provides and receives personal electronic health data under a priority category for primary use established under the EHDS Regulation in the European electronic health record exchange format"@en ;
    skos:prefLabel "Interoperability Software for EHR System"@en .

sector-health-owl:LifeInsuranceManagement a rdfs:Class,
        owl:Class,
        dpv-owl:Purpose ;
    dct:created "2024-12-01"^^xsd:date ;
    rdfs:isDefinedBy sector-health-owl: ;
    rdfs:subClassOf sector-health-owl:InsuranceManagement ;
    sw:term_status "accepted"@en ;
    skos:definition "Purposes associated with managing life insurance as part of healthcare services"@en ;
    skos:prefLabel "Life Insurance Management"@en .

sector-health-owl:LifestyleData a rdfs:Class,
        owl:Class,
        dpv-owl:PersonalData ;
    dct:contributor _:person-beatriz-esteves ;
    dct:created "2026-02-04"^^xsd:date ;
    rdfs:isDefinedBy sector-health-owl: ;
    rdfs:subClassOf pd-owl:Behavioural ;
    sw:term_status "accepted"@en ;
    skos:definition "Information about lifestyle"@en ;
    skos:prefLabel "Lifestyle Data"@en .

sector-health-owl:LipidomicData a rdfs:Class,
        owl:Class,
        dpv-owl:PersonalData ;
    dct:contributor _:person-beatriz-esteves ;
    dct:created "2026-02-04"^^xsd:date ;
    rdfs:isDefinedBy sector-health-owl: ;
    rdfs:subClassOf pd-owl:Molecular ;
    sw:term_status "accepted"@en ;
    skos:definition "Information about lipidomic data"@en ;
    skos:prefLabel "Lipidomic Data"@en .

sector-health-owl:LoggingSoftwareForEHRSystem a rdfs:Class,
        owl:Class,
        dpv-owl:Technology ;
    dct:contributor _:person-beatriz-esteves ;
    dct:created "2025-10-28"^^xsd:date ;
    rdfs:isDefinedBy sector-health-owl: ;
    rdfs:subClassOf tech-owl:Software ;
    sw:term_status "accepted"@en ;
    skos:definition "Software component of the EHR system which provides logging information related to access by health professionals or other individuals to priority categories of personal electronic health data"@en ;
    skos:prefLabel "Logging Software for EHR System"@en .

sector-health-owl:MedicalConditionDiagnosis a rdfs:Class,
        owl:Class,
        dpv-owl:Purpose ;
    dct:created "2024-12-01"^^xsd:date ;
    rdfs:isDefinedBy sector-health-owl: ;
    rdfs:subClassOf sector-health-owl:DiagnosisManagement ;
    sw:term_status "accepted"@en ;
    skos:definition "Purposes associated with conducting and managing medical diagnosis as part of healthcare services"@en ;
    skos:prefLabel "Medical Condition Diagnosis"@en .

sector-health-owl:MedicalDeviceManufacturer a rdfs:Class,
        owl:Class,
        dpv-owl:LegalEntity ;
    dct:contributor _:person-beatriz-esteves ;
    dct:created "2026-02-04"^^xsd:date ;
    dct:source "EHDS Art.27.1"@en ;
    rdfs:isDefinedBy sector-health-owl: ;
    rdfs:subClassOf tech-owl:Manufacturer ;
    sw:term_status "accepted"@en ;
    skos:definition "Actor that manufactures medical devices"@en ;
    skos:prefLabel "Medical Device Manufacturer"@en .

sector-health-owl:MedicalDevicesData a rdfs:Class,
        owl:Class,
        dpv-owl:PersonalData ;
    dct:contributor _:person-beatriz-esteves ;
    dct:created "2026-02-04"^^xsd:date ;
    rdfs:isDefinedBy sector-health-owl: ;
    rdfs:subClassOf pd-owl:MedicalHealth ;
    sw:term_status "accepted"@en ;
    skos:definition "Information about electronic health data from medical devices"@en ;
    skos:prefLabel "Medical Devices Data"@en .

sector-health-owl:MedicalDevicesDispensation a rdfs:Class,
        owl:Class,
        dpv-owl:Purpose ;
    dct:contributor _:person-beatriz-esteves ;
    dct:created "2025-10-28"^^xsd:date ;
    rdfs:isDefinedBy sector-health-owl: ;
    rdfs:subClassOf sector-health-owl:DispensationManagement ;
    sw:term_status "accepted"@en ;
    skos:definition "Purposes associated with the dispensation of medical devices"@en ;
    skos:prefLabel "Medical Devices Dispensation"@en .

sector-health-owl:MedicalDevicesPrescription a rdfs:Class,
        owl:Class,
        dpv-owl:Purpose ;
    dct:contributor _:person-beatriz-esteves ;
    dct:created "2025-10-28"^^xsd:date ;
    rdfs:isDefinedBy sector-health-owl: ;
    rdfs:subClassOf sector-health-owl:PrescriptionManagement ;
    sw:term_status "accepted"@en ;
    skos:definition "Purposes associated with prescription of medical devices"@en ;
    skos:prefLabel "Medical Devices Prescription"@en .

sector-health-owl:MedicalDevicesProvision a rdfs:Class,
        owl:Class,
        dpv-owl:Purpose ;
    dct:contributor _:person-beatriz-esteves ;
    dct:created "2025-10-28"^^xsd:date ;
    rdfs:isDefinedBy sector-health-owl: ;
    rdfs:subClassOf sector-health-owl:ServiceProvision ;
    sw:term_status "accepted"@en ;
    skos:definition "Purposes associated with the provision of medical devices"@en ;
    skos:prefLabel "Medical Devices Provision"@en .

sector-health-owl:MedicalDevicesRegistryData a rdfs:Class,
        owl:Class,
        dpv-owl:PersonalData ;
    dct:contributor _:person-beatriz-esteves ;
    dct:created "2026-02-04"^^xsd:date ;
    rdfs:isDefinedBy sector-health-owl: ;
    rdfs:subClassOf sector-health-owl:HealthRegistryData ;
    sw:term_status "accepted"@en ;
    skos:definition "Information about electronic health data from registries for medical devices"@en ;
    skos:prefLabel "Medical Devices Registry Data"@en .

sector-health-owl:MedicalImaging a rdfs:Class,
        owl:Class,
        dpv-owl:PersonalData ;
    dct:contributor _:person-beatriz-esteves ;
    dct:created "2025-10-28"^^xsd:date ;
    rdfs:isDefinedBy sector-health-owl: ;
    rdfs:subClassOf pd-owl:HealthRecord ;
    sw:term_status "accepted"@en ;
    skos:definition "Information about medical imaging studies and related imaging reports"@en ;
    skos:prefLabel "Medical Imaging"@en .

sector-health-owl:MedicalRegistryData a rdfs:Class,
        owl:Class,
        dpv-owl:PersonalData ;
    dct:contributor _:person-beatriz-esteves ;
    dct:created "2026-02-04"^^xsd:date ;
    rdfs:isDefinedBy sector-health-owl: ;
    rdfs:subClassOf sector-health-owl:HealthRegistryData ;
    sw:term_status "accepted"@en ;
    skos:definition "Information about electronic health data from medical registries"@en ;
    skos:prefLabel "Medical Registry Data"@en .

sector-health-owl:MedicalResourceOptimisation a rdfs:Class,
        owl:Class,
        dpv-owl:Purpose ;
    dct:created "2024-12-01"^^xsd:date ;
    rdfs:isDefinedBy sector-health-owl: ;
    rdfs:subClassOf sector-health-owl:Optimisation ;
    sw:term_status "accepted"@en ;
    skos:definition "Purposes associated with identifying optimisations related to use of medical resources as part of healthcare services"@en ;
    skos:prefLabel "Medical Resource Optimisation"@en .

sector-health-owl:MedicalTestResult a rdfs:Class,
        owl:Class,
        dpv-owl:PersonalData ;
    dct:contributor _:person-beatriz-esteves ;
    dct:created "2025-10-28"^^xsd:date ;
    rdfs:isDefinedBy sector-health-owl: ;
    rdfs:subClassOf pd-owl:HealthRecord ;
    sw:term_status "accepted"@en ;
    skos:definition "Information about medical test results"@en ;
    skos:prefLabel "Medical Test Result"@en .

sector-health-owl:MedicinalProductsDispensation a rdfs:Class,
        owl:Class,
        dpv-owl:Purpose ;
    dct:contributor _:person-beatriz-esteves ;
    dct:created "2025-10-28"^^xsd:date ;
    rdfs:isDefinedBy sector-health-owl: ;
    rdfs:subClassOf sector-health-owl:DispensationManagement ;
    sw:term_status "accepted"@en ;
    skos:definition "Purposes associated with the dispensation of medicinal products"@en ;
    skos:prefLabel "Medicinal Products Dispensation"@en .

sector-health-owl:MedicinalProductsPrescription a rdfs:Class,
        owl:Class,
        dpv-owl:Purpose ;
    dct:contributor _:person-beatriz-esteves ;
    dct:created "2025-10-28"^^xsd:date ;
    rdfs:isDefinedBy sector-health-owl: ;
    rdfs:subClassOf sector-health-owl:PrescriptionManagement ;
    sw:term_status "accepted"@en ;
    skos:definition "Purposes associated with prescription of medicinal products"@en ;
    skos:prefLabel "Medicinal Products Prescription"@en .

sector-health-owl:MedicinalProductsProvision a rdfs:Class,
        owl:Class,
        dpv-owl:Purpose ;
    dct:contributor _:person-beatriz-esteves ;
    dct:created "2025-10-28"^^xsd:date ;
    rdfs:isDefinedBy sector-health-owl: ;
    rdfs:subClassOf sector-health-owl:ServiceProvision ;
    sw:term_status "accepted"@en ;
    skos:definition "Purposes associated with the provision of medicinal products"@en ;
    skos:prefLabel "Medicinal Products Provision"@en .

sector-health-owl:MedicinalProductsRegistryData a rdfs:Class,
        owl:Class,
        dpv-owl:PersonalData ;
    dct:contributor _:person-beatriz-esteves ;
    dct:created "2026-02-04"^^xsd:date ;
    rdfs:isDefinedBy sector-health-owl: ;
    rdfs:subClassOf sector-health-owl:HealthRegistryData ;
    sw:term_status "accepted"@en ;
    skos:definition "Information about electronic health data from registries for medicinal products"@en ;
    skos:prefLabel "Medicinal Products Registry Data"@en .

sector-health-owl:MentalHealthAwareness a rdfs:Class,
        owl:Class,
        dpv-owl:Purpose ;
    dct:created "2024-12-01"^^xsd:date ;
    rdfs:isDefinedBy sector-health-owl: ;
    rdfs:subClassOf sector-health-owl:PreventativeCareManagement ;
    sw:term_status "accepted"@en ;
    skos:definition "Purposes associated with management of mental health awareness as part of healthcare services"@en ;
    skos:prefLabel "Mental Health Awareness"@en .

sector-health-owl:MentalHealthConditionDiagnosis a rdfs:Class,
        owl:Class,
        dpv-owl:Purpose ;
    dct:created "2024-12-01"^^xsd:date ;
    rdfs:isDefinedBy sector-health-owl: ;
    rdfs:subClassOf sector-health-owl:DiagnosisManagement ;
    sw:term_status "accepted"@en ;
    skos:definition "Purposes associated with conducting and managing mental health diagnosis as part of healthcare services"@en ;
    skos:prefLabel "Mental Health Condition Diagnosis"@en .

sector-health-owl:MetabolomicData a rdfs:Class,
        owl:Class,
        dpv-owl:PersonalData ;
    dct:contributor _:person-beatriz-esteves ;
    dct:created "2026-02-04"^^xsd:date ;
    rdfs:isDefinedBy sector-health-owl: ;
    rdfs:subClassOf pd-owl:Molecular ;
    sw:term_status "accepted"@en ;
    skos:definition "Information about metabolomic data"@en ;
    skos:prefLabel "Metabolomic Data"@en .

sector-health-owl:MortalityRegistryData a rdfs:Class,
        owl:Class,
        dpv-owl:PersonalData ;
    dct:contributor _:person-beatriz-esteves ;
    dct:created "2026-02-04"^^xsd:date ;
    rdfs:isDefinedBy sector-health-owl: ;
    rdfs:subClassOf sector-health-owl:HealthRegistryData ;
    sw:term_status "accepted"@en ;
    skos:definition "Information about electronic health data from mortality registries"@en ;
    skos:prefLabel "Mortality Registry Data"@en .

sector-health-owl:NonPersonalElectronicHealthData a rdfs:Class,
        owl:Class,
        dpv-owl:NonPersonalData ;
    dct:contributor _:person-beatriz-esteves ;
    dct:created "2025-10-28"^^xsd:date ;
    rdfs:isDefinedBy sector-health-owl: ;
    rdfs:subClassOf sector-health-owl:ElectronicHealthData ;
    sw:term_status "accepted"@en ;
    skos:definition "Information about electronic health data that is not personal data, including anonymised data"@en ;
    skos:prefLabel "Non-Personal Electronic Health Data"@en .

sector-health-owl:Optimisation a rdfs:Class,
        owl:Class,
        dpv-owl:Purpose ;
    dct:created "2024-12-01"^^xsd:date ;
    rdfs:isDefinedBy sector-health-owl: ;
    rdfs:subClassOf dpv-owl:ImproveHealthcare,
        sector-health-owl:HealthcareManagement ;
    sw:term_status "accepted"@en ;
    skos:definition "Purposes associated with identifying optimisations to use and provision of healthcare services"@en ;
    skos:prefLabel "Optimisation"@en .

sector-health-owl:PandemicResponseManagement a rdfs:Class,
        owl:Class,
        dpv-owl:Purpose ;
    dct:created "2024-12-01"^^xsd:date ;
    rdfs:isDefinedBy sector-health-owl: ;
    rdfs:subClassOf sector-health-owl:CrisisManagement ;
    sw:term_status "accepted"@en ;
    skos:definition "Purposes associated with management of pandemics and related crisis situations in relation to healthcare services"@en ;
    skos:prefLabel "Pandemic Response Management"@en .

sector-health-owl:PathogenData a rdfs:Class,
        owl:Class,
        dpv-owl:NonPersonalData ;
    dct:contributor _:person-beatriz-esteves ;
    dct:created "2026-02-04"^^xsd:date ;
    rdfs:isDefinedBy sector-health-owl: ;
    rdfs:subClassOf dpv-owl:NonPersonalData ;
    sw:term_status "accepted"@en ;
    skos:definition "Information about relevant pathogen data, impacting on human health"@en ;
    skos:prefLabel "Pathogen Data"@en .

sector-health-owl:PatientChronicConditionMonitoring a rdfs:Class,
        owl:Class,
        dpv-owl:Purpose ;
    dct:created "2024-12-01"^^xsd:date ;
    rdfs:isDefinedBy sector-health-owl: ;
    rdfs:subClassOf sector-health-owl:PatientMonitoring ;
    sw:term_status "accepted"@en ;
    skos:definition "Purposes associated with monitoring of patients with chronic conditions for health and safety as part of healthcare services"@en ;
    skos:prefLabel "Patient Chronic Condition Monitoring"@en .

sector-health-owl:PatientConsentManagement a rdfs:Class,
        owl:Class,
        dpv-owl:Purpose ;
    dct:created "2024-12-01"^^xsd:date ;
    rdfs:isDefinedBy sector-health-owl: ;
    rdfs:subClassOf sector-health-owl:PatientInformationManagement ;
    sw:term_status "accepted"@en ;
    skos:definition "Purposes associated with management of consent from or related to patients in relation to healthcare services"@en ;
    skos:prefLabel "Patient Consent Management"@en .

sector-health-owl:PatientInformationManagement a rdfs:Class,
        owl:Class,
        dpv-owl:Purpose ;
    dct:created "2024-12-01"^^xsd:date ;
    rdfs:isDefinedBy sector-health-owl: ;
    rdfs:subClassOf sector-health-owl:ResourceManagement ;
    sw:term_status "accepted"@en ;
    skos:definition "Purposes associated with management of patient information in relation to healthcare services"@en ;
    skos:prefLabel "Patient Information Management"@en .

sector-health-owl:PatientIntensiveCareMonitoring a rdfs:Class,
        owl:Class,
        dpv-owl:Purpose ;
    dct:created "2024-12-01"^^xsd:date ;
    rdfs:isDefinedBy sector-health-owl: ;
    rdfs:subClassOf sector-health-owl:PatientMonitoring ;
    sw:term_status "accepted"@en ;
    skos:definition "Purposes associated with monitoring of patients in intensive care as part of healthcare services"@en ;
    skos:prefLabel "Patient Intensive Care Monitoring"@en .

sector-health-owl:PatientMonitoring a rdfs:Class,
        owl:Class,
        dpv-owl:Purpose ;
    dct:created "2024-12-01"^^xsd:date ;
    rdfs:isDefinedBy sector-health-owl: ;
    rdfs:subClassOf sector-health-owl:ServiceProvision ;
    sw:term_status "accepted"@en ;
    skos:definition "Purposes associated with monitoring of patients for treatment and safety as part of healthcare services"@en ;
    skos:prefLabel "Patient Monitoring"@en .

sector-health-owl:PatientPostTreatmentMonitoring a rdfs:Class,
        owl:Class,
        dpv-owl:Purpose ;
    dct:created "2024-12-01"^^xsd:date ;
    rdfs:isDefinedBy sector-health-owl: ;
    rdfs:subClassOf sector-health-owl:PatientMonitoring ;
    sw:term_status "accepted"@en ;
    skos:definition "Purposes associated with monitoring of patients post-treatment for health and safety as part of healthcare services"@en ;
    skos:prefLabel "Patient Post Treatment Monitoring"@en .

sector-health-owl:PatientRemoteMonitoring a rdfs:Class,
        owl:Class,
        dpv-owl:Purpose ;
    dct:created "2024-12-01"^^xsd:date ;
    rdfs:isDefinedBy sector-health-owl: ;
    rdfs:subClassOf sector-health-owl:PatientMonitoring ;
    sw:term_status "accepted"@en ;
    skos:definition "Purposes associated with remote monitoring of patients for treatment and safety as part of healthcare services"@en ;
    skos:prefLabel "Patient Remote Monitoring"@en .

sector-health-owl:PatientSummary a rdfs:Class,
        owl:Class,
        dpv-owl:PersonalData ;
    dct:contributor _:person-beatriz-esteves ;
    dct:created "2025-10-28"^^xsd:date ;
    rdfs:isDefinedBy sector-health-owl: ;
    rdfs:subClassOf pd-owl:HealthRecord ;
    sw:term_status "accepted"@en ;
    skos:definition "Information about patient summaries"@en ;
    skos:prefLabel "Patient Summary"@en .

sector-health-owl:PatientTreatmentEffectivenessMonitoring a rdfs:Class,
        owl:Class,
        dpv-owl:Purpose ;
    dct:created "2024-12-01"^^xsd:date ;
    rdfs:isDefinedBy sector-health-owl: ;
    rdfs:subClassOf sector-health-owl:PatientMonitoring ;
    sw:term_status "accepted"@en ;
    skos:definition "Purposes associated with monitoring of treatment effectiveness as part of healthcare services"@en ;
    skos:prefLabel "Patient Treatment Effectiveness Monitoring"@en .

sector-health-owl:PatientTreatmentOutcomeAnalysis a rdfs:Class,
        owl:Class,
        dpv-owl:Purpose ;
    dct:created "2024-12-01"^^xsd:date ;
    rdfs:isDefinedBy sector-health-owl: ;
    rdfs:subClassOf sector-health-owl:PatientMonitoring ;
    sw:term_status "accepted"@en ;
    skos:definition "Purposes associated with analysis of patient treatment outcomes as part of healthcare services"@en ;
    skos:prefLabel "Patient Treatment Outcome Analysis"@en .

sector-health-owl:PerformanceStudiesData a rdfs:Class,
        owl:Class,
        dpv-owl:PersonalData ;
    dct:contributor _:person-beatriz-esteves ;
    dct:created "2026-02-04"^^xsd:date ;
    rdfs:isDefinedBy sector-health-owl: ;
    rdfs:subClassOf sector-health-owl:StudyData ;
    sw:term_status "accepted"@en ;
    skos:definition "Information about health data from performance studies"@en ;
    skos:prefLabel "Performance Studies Data"@en .

sector-health-owl:PersonGeneratedHealthAppData a rdfs:Class,
        owl:Class,
        dpv-owl:PersonalData ;
    dct:contributor _:person-beatriz-esteves ;
    dct:created "2026-02-04"^^xsd:date ;
    rdfs:isDefinedBy sector-health-owl: ;
    rdfs:subClassOf sector-health-owl:PersonGeneratedHealthData ;
    sw:term_status "accepted"@en ;
    skos:definition "Information about person generated digital health applications data"@en ;
    skos:prefLabel "Person Generated Health Application Data"@en .

sector-health-owl:PersonGeneratedHealthData a rdfs:Class,
        owl:Class,
        dpv-owl:PersonalData ;
    dct:contributor _:person-beatriz-esteves ;
    dct:created "2026-02-04"^^xsd:date ;
    rdfs:isDefinedBy sector-health-owl: ;
    rdfs:subClassOf pd-owl:MedicalHealth ;
    sw:term_status "accepted"@en ;
    skos:definition "Information about person generated electronic health data"@en ;
    skos:prefLabel "Person Generated Health Data"@en .

sector-health-owl:PersonGeneratedMedicalDeviceData a rdfs:Class,
        owl:Class,
        dpv-owl:PersonalData ;
    dct:contributor _:person-beatriz-esteves ;
    dct:created "2026-02-04"^^xsd:date ;
    rdfs:isDefinedBy sector-health-owl: ;
    rdfs:subClassOf sector-health-owl:PersonGeneratedHealthData ;
    sw:term_status "accepted"@en ;
    skos:definition "Information about person generated medical devices data"@en ;
    skos:prefLabel "Person Generated Medical Devices Data"@en .

sector-health-owl:PersonGeneratedWellnessAppData a rdfs:Class,
        owl:Class,
        dpv-owl:PersonalData ;
    dct:contributor _:person-beatriz-esteves ;
    dct:created "2026-02-04"^^xsd:date ;
    rdfs:isDefinedBy sector-health-owl: ;
    rdfs:subClassOf sector-health-owl:PersonGeneratedHealthAppData ;
    sw:term_status "accepted"@en ;
    skos:definition "Information about person generated wellness applications data"@en ;
    skos:prefLabel "Person Generated Wellness Application Data"@en .

sector-health-owl:PersonalElectronicHealthData a rdfs:Class,
        owl:Class,
        dpv-owl:PersonalData ;
    dct:contributor _:person-beatriz-esteves ;
    dct:created "2025-10-28"^^xsd:date ;
    rdfs:isDefinedBy sector-health-owl: ;
    rdfs:subClassOf sector-health-owl:ElectronicHealthData ;
    sw:term_status "accepted"@en ;
    skos:definition "Information about personal health data, including genetic data, processed in an electronic form"@en ;
    skos:prefLabel "Personal Electronic Health Data"@en .

sector-health-owl:PersonalisedHealthcare a rdfs:Class,
        owl:Class,
        dpv-owl:Purpose ;
    dct:contributor _:person-beatriz-esteves ;
    dct:created "2026-02-04"^^xsd:date ;
    rdfs:isDefinedBy sector-health-owl: ;
    rdfs:subClassOf dpv-owl:ImproveHealthcare,
        dpv-owl:Personalisation ;
    sw:term_status "accepted"@en ;
    skos:definition "Purposes associated with providing personalised healthcare"@en ;
    skos:prefLabel "Personalised Healthcare"@en .

sector-health-owl:PopulationHealthAnalysis a rdfs:Class,
        owl:Class,
        dpv-owl:Purpose ;
    dct:created "2024-12-01"^^xsd:date ;
    rdfs:isDefinedBy sector-health-owl: ;
    rdfs:subClassOf sector-health-owl:ResearchDevelopment ;
    sw:term_status "accepted"@en ;
    skos:definition "Purposes associated with analysing trends and outcomes in a specific population or group of people regarding health and safety"@en ;
    skos:prefLabel "Population Health Analysis"@en .

sector-health-owl:PredictiveHealthRiskAnalysis a rdfs:Class,
        owl:Class,
        dpv-owl:Purpose ;
    dct:created "2024-12-01"^^xsd:date ;
    rdfs:isDefinedBy sector-health-owl: ;
    rdfs:subClassOf sector-health-owl:ResearchDevelopment ;
    sw:term_status "accepted"@en ;
    skos:definition "Purposes associated with analysing and predicting risks to public health and safety"@en ;
    skos:prefLabel "Predictive Health Risk Analysis"@en .

sector-health-owl:PrescriptionManagement a rdfs:Class,
        owl:Class,
        dpv-owl:Purpose ;
    dct:contributor _:person-beatriz-esteves ;
    dct:created "2025-10-28"^^xsd:date ;
    rdfs:isDefinedBy sector-health-owl: ;
    rdfs:subClassOf sector-health-owl:ServiceProvision ;
    sw:term_status "accepted"@en ;
    skos:definition "Purposes associated with prescription of products, devices and other healthcare-related resources"@en ;
    skos:prefLabel "Prescription Management"@en .

sector-health-owl:PreventativeCareManagement a rdfs:Class,
        owl:Class,
        dpv-owl:Purpose ;
    dct:created "2024-12-01"^^xsd:date ;
    rdfs:isDefinedBy sector-health-owl: ;
    rdfs:subClassOf dpv-owl:ImproveHealthcare,
        sector-health-owl:HealthcareServiceManagement ;
    sw:term_status "accepted"@en ;
    skos:definition "Purposes associated with management of preventative care as part of healthcare services"@en ;
    skos:prefLabel "Preventative Care Management"@en .

sector-health-owl:PrimaryCareManagement a rdfs:Class,
        owl:Class,
        dpv-owl:Purpose ;
    dct:created "2024-12-01"^^xsd:date ;
    rdfs:isDefinedBy sector-health-owl: ;
    rdfs:subClassOf sector-health-owl:HealthcareServiceManagement ;
    sw:term_status "accepted"@en ;
    skos:definition "Purposes associated with management of primary healthcare services"@en ;
    skos:prefLabel "Primary Care Management"@en .

sector-health-owl:PrimaryUse a rdfs:Class,
        owl:Class,
        sector-health-owl:ReuseCompatibility ;
    dct:contributor _:person-arthit-suriyawongkul,
        _:person-beatriz-esteves,
        _:person-delaram-golpayegani,
        _:person-georg-p-krog,
        _:person-harshvardhan-j-pandit,
        _:person-julian-flake ;
    dct:created "2025-06-19"^^xsd:date ;
    rdfs:isDefinedBy sector-health-owl: ;
    rdfs:subClassOf dpv-owl:PrimaryUse ;
    sw:term_status "accepted"@en ;
    skos:definition "Status indicating the reuse of health is compatible with the original purpose or use i.e. it can be considered as 'Primary Use'"@en ;
    skos:prefLabel "Primary Use"@en ;
    skos:scopeNote "Primary Use refers to an assessment where two contexts are found to be compatible, e.g. if purpose is used to test compatibility, then for two activities the second activity is said be the primary use if its purpose is compatible with the first activity's purpose"@en .

sector-health-owl:ProtectAgainstCrossBorderThreatsToHealth a rdfs:Class,
        owl:Class,
        dpv-owl:Purpose ;
    dct:contributor _:person-beatriz-esteves ;
    dct:created "2026-02-04"^^xsd:date ;
    rdfs:isDefinedBy sector-health-owl: ;
    rdfs:subClassOf sector-health-owl:PublicInterestRelatedToHealth ;
    sw:term_status "accepted"@en ;
    skos:definition "Purposes associated with the protection against serious cross-border threats to health"@en ;
    skos:prefLabel "Protect against Cross-border Threats to Health"@en .

sector-health-owl:ProteomicData a rdfs:Class,
        owl:Class,
        dpv-owl:PersonalData ;
    dct:contributor _:person-beatriz-esteves ;
    dct:created "2026-02-04"^^xsd:date ;
    rdfs:isDefinedBy sector-health-owl: ;
    rdfs:subClassOf pd-owl:Molecular ;
    sw:term_status "accepted"@en ;
    skos:definition "Information about proteomic data"@en ;
    skos:prefLabel "Proteomic Data"@en .

sector-health-owl:ProvideHealthcareOfficialStatistics a rdfs:Class,
        owl:Class,
        dpv-owl:Purpose ;
    dct:contributor _:person-beatriz-esteves ;
    dct:created "2026-02-04"^^xsd:date ;
    rdfs:isDefinedBy sector-health-owl: ;
    rdfs:subClassOf dpv-owl:ProvideOfficialStatistics ;
    sw:term_status "accepted"@en ;
    skos:definition "Purposes associated with facilitating the development, production and dissemination of reliable official statistics related to health or care sectors"@en ;
    skos:prefLabel "Provide Healthcare Official Statistics"@en .

sector-health-owl:ProvidersDataSharing a rdfs:Class,
        owl:Class,
        dpv-owl:Purpose ;
    dct:created "2024-12-01"^^xsd:date ;
    rdfs:isDefinedBy sector-health-owl: ;
    rdfs:subClassOf sector-health-owl:HealthcareServiceManagement ;
    sw:term_status "accepted"@en ;
    skos:definition "Purposes associated with sharing of patient information between healthcare providers, such as between hospitals treating the same patient"@en ;
    skos:prefLabel "Providers Data Sharing"@en .

sector-health-owl:PublicHealthMonitoring a rdfs:Class,
        owl:Class,
        dpv-owl:Purpose ;
    dct:created "2024-12-01"^^xsd:date ;
    rdfs:isDefinedBy sector-health-owl: ;
    rdfs:subClassOf sector-health-owl:PreventativeCareManagement ;
    sw:term_status "accepted"@en ;
    skos:definition "Purposes associated with monitoring of public health as part of healthcare services"@en ;
    skos:prefLabel "Public Health Monitoring"@en .

sector-health-owl:PublicHealthRegistryData a rdfs:Class,
        owl:Class,
        dpv-owl:PersonalData ;
    dct:contributor _:person-beatriz-esteves ;
    dct:created "2026-02-04"^^xsd:date ;
    rdfs:isDefinedBy sector-health-owl: ;
    rdfs:subClassOf sector-health-owl:HealthRegistryData ;
    sw:term_status "accepted"@en ;
    skos:definition "Information about registries of public health data"@en ;
    skos:prefLabel "Public Health Registry Data"@en .

sector-health-owl:PublicHealthSurveillance a rdfs:Class,
        owl:Class,
        dpv-owl:Purpose ;
    dct:contributor _:person-beatriz-esteves ;
    dct:created "2026-02-04"^^xsd:date ;
    rdfs:isDefinedBy sector-health-owl: ;
    rdfs:subClassOf sector-health-owl:PublicInterestRelatedToHealth ;
    sw:term_status "accepted"@en ;
    skos:definition "Purposes associated with public health surveillance"@en ;
    skos:prefLabel "Public Health Surveillance"@en .

sector-health-owl:PublicInterestRelatedToHealth a rdfs:Class,
        owl:Class,
        dpv-owl:Purpose ;
    dct:contributor _:person-beatriz-esteves ;
    dct:created "2026-02-04"^^xsd:date ;
    rdfs:isDefinedBy sector-health-owl: ;
    rdfs:subClassOf dpv-owl:Purpose ;
    sw:term_status "accepted"@en ;
    skos:definition "Purposes associated with pursuing activities for reasons of public interest in the area of public and occupational health"@en ;
    skos:prefLabel "Public Interest related to Health"@en .

sector-health-owl:PublicPolicyMaking a rdfs:Class,
        owl:Class,
        dpv-owl:Purpose ;
    dct:contributor _:person-beatriz-esteves ;
    dct:created "2026-02-04"^^xsd:date ;
    rdfs:isDefinedBy sector-health-owl: ;
    rdfs:subClassOf dpv-owl:PublicPolicyMaking ;
    sw:term_status "accepted"@en ;
    skos:definition "Purposes associated with public policy making policymaking in the healthcare sector"@en ;
    skos:prefLabel "Public Policy Making"@en .

sector-health-owl:ReferralManagement a rdfs:Class,
        owl:Class,
        dpv-owl:Purpose ;
    dct:created "2024-12-01"^^xsd:date ;
    rdfs:isDefinedBy sector-health-owl: ;
    rdfs:subClassOf sector-health-owl:HealthcareServiceManagement ;
    sw:term_status "accepted"@en ;
    skos:definition "Purposes associated with management of referrals as part of healthcare services"@en ;
    skos:prefLabel "Referral Management"@en .

sector-health-owl:ReimbursementAdminData a rdfs:Class,
        owl:Class,
        dpv-owl:PersonalData ;
    dct:contributor _:person-beatriz-esteves ;
    dct:created "2026-02-04"^^xsd:date ;
    rdfs:isDefinedBy sector-health-owl: ;
    rdfs:subClassOf sector-health-owl:HealthAdminData ;
    sw:term_status "accepted"@en ;
    skos:definition "Information about health-related administrative data on reimbursements"@en ;
    skos:prefLabel "Health-related Administrative Data on Reimbursements"@en .

sector-health-owl:ReimbursementServicesProvision a rdfs:Class,
        owl:Class,
        dpv-owl:Purpose ;
    dct:contributor _:person-beatriz-esteves ;
    dct:created "2025-10-28"^^xsd:date ;
    rdfs:isDefinedBy sector-health-owl: ;
    rdfs:subClassOf sector-health-owl:ServiceProvision ;
    sw:term_status "accepted"@en ;
    skos:definition "Purposes associated with the provision of reimbursement services related to healthcare"@en ;
    skos:prefLabel "Reimbursement Services Provision"@en .

sector-health-owl:ResearchCohortData a rdfs:Class,
        owl:Class,
        dpv-owl:PersonalData ;
    dct:contributor _:person-beatriz-esteves ;
    dct:created "2026-02-04"^^xsd:date ;
    rdfs:isDefinedBy sector-health-owl: ;
    rdfs:subClassOf sector-health-owl:StudyData ;
    sw:term_status "accepted"@en ;
    skos:definition "Information about health data from research cohorts"@en ;
    skos:prefLabel "Research Cohort Data"@en .

sector-health-owl:ResearchDevelopment a rdfs:Class,
        owl:Class,
        dpv-owl:Purpose ;
    dct:created "2024-12-01"^^xsd:date ;
    rdfs:isDefinedBy sector-health-owl: ;
    rdfs:subClassOf dpv-owl:ImproveHealthcare,
        dpv-owl:ResearchAndDevelopment,
        sector-health-owl:HealthcareManagement ;
    sw:term_status "accepted"@en ;
    skos:definition "Purposes associated with research and development regarding healthcare services"@en ;
    skos:prefLabel "Research Development"@en .

sector-health-owl:ResourceManagement a rdfs:Class,
        owl:Class,
        dpv-owl:Purpose ;
    dct:created "2024-12-01"^^xsd:date ;
    rdfs:isDefinedBy sector-health-owl: ;
    rdfs:subClassOf sector-health-owl:HealthcareManagement ;
    sw:term_status "accepted"@en ;
    skos:definition "Purposes associated with management of resources related to healthcare services"@en ;
    skos:prefLabel "Resource Management"@en .

sector-health-owl:ReuseCompatibility a rdfs:Class,
        owl:Class ;
    dct:contributor _:person-arthit-suriyawongkul,
        _:person-beatriz-esteves,
        _:person-delaram-golpayegani,
        _:person-georg-p-krog,
        _:person-harshvardhan-j-pandit,
        _:person-julian-flake ;
    dct:created "2025-06-19"^^xsd:date ;
    rdfs:isDefinedBy sector-health-owl: ;
    rdfs:subClassOf dpv-owl:ReuseCompatibility ;
    sw:term_status "accepted"@en ;
    skos:definition "Status indicating whether the reuse of health data is compatible for given context"@en ;
    skos:prefLabel "ReuseCompatibility"@en ;
    skos:scopeNote "Compatibility refers to whether two contexts, such as dpv:Process instances, are compatible with each other based on a criteria which is not defined by the concept. This criteria can be based on requirements from law, such as GDPR's purpose compatibility or can be based on privacy norms such as contextual integrity. To express such interpretations, further concepts should be expanded from this base concept"@en .

sector-health-owl:SecondMedicalOpinion a rdfs:Class,
        owl:Class,
        dpv-owl:Purpose ;
    dct:contributor _:person-beatriz-esteves ;
    dct:created "2025-10-28"^^xsd:date ;
    rdfs:isDefinedBy sector-health-owl: ;
    rdfs:subClassOf sector-health-owl:HealthcareServiceManagement ;
    sw:term_status "accepted"@en ;
    skos:definition "Purposes associated with the management of a consultation with a healthcare professional other than the initial one to review a diagnosis or treatment plan"@en ;
    skos:prefLabel "Second Medical Opinion"@en .

sector-health-owl:SecondaryUse a rdfs:Class,
        owl:Class,
        sector-health-owl:ReuseCompatibility ;
    dct:contributor _:person-arthit-suriyawongkul,
        _:person-beatriz-esteves,
        _:person-delaram-golpayegani,
        _:person-georg-p-krog,
        _:person-harshvardhan-j-pandit,
        _:person-julian-flake ;
    dct:created "2025-06-19"^^xsd:date ;
    rdfs:isDefinedBy sector-health-owl: ;
    rdfs:subClassOf dpv-owl:SecondaryUse ;
    sw:term_status "accepted"@en ;
    skos:definition "Status indicating the reuse of health is incompatible with the original purpose or use i.e. it is considered as 'Secondary Use'"@en ;
    skos:prefLabel "Secondary Use"@en ;
    skos:scopeNote "Secondary Use refers to an assessment where two contexts are found to be incompatible, e.g. if purpose is used to test compatibility, then for two activities the second activity is said be the secondary use if its purpose is incompatible with the first activity's purpose"@en .

sector-health-owl:SecurityManagement a rdfs:Class,
        owl:Class,
        dpv-owl:Purpose ;
    dct:created "2024-12-01"^^xsd:date ;
    rdfs:isDefinedBy sector-health-owl: ;
    rdfs:subClassOf dpv-owl:OrganisationRiskManagement,
        sector-health-owl:HealthcareManagement ;
    sw:term_status "accepted"@en ;
    skos:definition "Purposes associated with management of security in relation to healthcare services"@en ;
    skos:prefLabel "Security Management"@en .

sector-health-owl:ServiceBillingFraudManagement a rdfs:Class,
        owl:Class,
        dpv-owl:Purpose ;
    dct:created "2024-12-01"^^xsd:date ;
    rdfs:isDefinedBy sector-health-owl: ;
    rdfs:subClassOf sector-health-owl:FraudPreventionDetection ;
    sw:term_status "accepted"@en ;
    skos:definition "Purposes associated with billing prevention and detection in relation to healthcare services"@en ;
    skos:prefLabel "Service Billing Fraud Management"@en .

sector-health-owl:ServiceProvision a rdfs:Class,
        owl:Class,
        dpv-owl:Purpose ;
    dct:created "2024-12-01"^^xsd:date ;
    rdfs:isDefinedBy sector-health-owl: ;
    rdfs:subClassOf dpv-owl:ServiceProvision,
        sector-health-owl:HealthcareServiceManagement ;
    sw:term_status "accepted"@en ;
    skos:definition "Purposes associated with provision of healthcare services"@en ;
    skos:prefLabel "Service Provision"@en .

sector-health-owl:SocialServicesProvision a rdfs:Class,
        owl:Class,
        dpv-owl:Purpose ;
    dct:contributor _:person-beatriz-esteves ;
    dct:created "2025-10-28"^^xsd:date ;
    rdfs:isDefinedBy sector-health-owl: ;
    rdfs:subClassOf sector-health-owl:ServiceProvision ;
    sw:term_status "accepted"@en ;
    skos:definition "Purposes associated with the provision of social services related to healthcare"@en ;
    skos:prefLabel "Social Services Provision"@en .

sector-health-owl:SocioeconomicHealthDeterminant a rdfs:Class,
        owl:Class,
        dpv-owl:PersonalData ;
    dct:contributor _:person-beatriz-esteves ;
    dct:created "2026-02-04"^^xsd:date ;
    rdfs:isDefinedBy sector-health-owl: ;
    rdfs:subClassOf pd-owl:Health ;
    sw:term_status "accepted"@en ;
    skos:definition "Information about socioeconomic data impacting on health"@en ;
    skos:prefLabel "Socioeconomic Health Determinant"@en .

sector-health-owl:SpecialisedCareManagement a rdfs:Class,
        owl:Class,
        dpv-owl:Purpose ;
    dct:created "2024-12-01"^^xsd:date ;
    rdfs:isDefinedBy sector-health-owl: ;
    rdfs:subClassOf sector-health-owl:HealthcareServiceManagement ;
    sw:term_status "accepted"@en ;
    skos:definition "Purposes associated with management of specialised healthcare services"@en ;
    skos:prefLabel "Specialised Care Management"@en .

sector-health-owl:StudyData a rdfs:Class,
        owl:Class,
        dpv-owl:PersonalData ;
    dct:contributor _:person-beatriz-esteves ;
    dct:created "2026-02-04"^^xsd:date ;
    rdfs:isDefinedBy sector-health-owl: ;
    rdfs:subClassOf pd-owl:MedicalHealth ;
    sw:term_status "accepted"@en ;
    skos:definition "Information about health data from studies, e.g. clinical trials, research cohorts, ..."@en ;
    skos:prefLabel "Study Data"@en .

sector-health-owl:SupportAuthoritiesRegulatoryActivities a rdfs:Class,
        owl:Class,
        dpv-owl:Purpose ;
    dct:contributor _:person-beatriz-esteves ;
    dct:created "2026-02-04"^^xsd:date ;
    rdfs:isDefinedBy sector-health-owl: ;
    rdfs:subClassOf dpv-owl:LegalCompliance ;
    sw:term_status "accepted"@en ;
    skos:definition "Purposes associated with supporting authorities to carry out their regulatory tasks"@en ;
    skos:prefLabel "Support Authorities in Regulatory Activities"@en .

sector-health-owl:System a rdfs:Class,
        owl:Class,
        dpv-owl:Technology ;
    dct:contributor _:person-beatriz-esteves ;
    dct:created "2025-10-28"^^xsd:date ;
    rdfs:isDefinedBy sector-health-owl: ;
    rdfs:subClassOf tech-owl:System ;
    sw:term_status "accepted"@en ;
    skos:definition "A system whereby the software and/or hardware allows personal electronic health data to be collected and processed, to be used by healthcare providers when providing patient care or by patients when accessing their electronic health data"@en ;
    skos:prefLabel "Electronic Health Record System"@en .

sector-health-owl:TrainTestAndEvaluateAISystemsAlgorithms a rdfs:Class,
        owl:Class,
        dpv-owl:Purpose ;
    dct:contributor _:person-beatriz-esteves ;
    dct:created "2026-02-04"^^xsd:date ;
    rdfs:isDefinedBy sector-health-owl: ;
    rdfs:subClassOf sector-health-owl:TrainTestAndEvaluateHealthAlgorithms ;
    sw:term_status "accepted"@en ;
    skos:definition "Purposes associated with training, testing and evaluating algorithms in AI systems"@en ;
    skos:prefLabel "Train, Test and Evaluate AI Systems Algorithms"@en .

sector-health-owl:TrainTestAndEvaluateHealthAlgorithms a rdfs:Class,
        owl:Class,
        dpv-owl:Purpose ;
    dct:contributor _:person-beatriz-esteves ;
    dct:created "2026-02-04"^^xsd:date ;
    rdfs:isDefinedBy sector-health-owl: ;
    rdfs:subClassOf dpv-owl:Purpose ;
    sw:term_status "accepted"@en ;
    skos:definition "Purposes associated with training, testing and evaluating health-related algorithms"@en ;
    skos:prefLabel "Train, Test and Evaluate Health-related Algorithms"@en .

sector-health-owl:TrainTestAndEvaluateHealthAppsAlgorithms a rdfs:Class,
        owl:Class,
        dpv-owl:Purpose ;
    dct:contributor _:person-beatriz-esteves ;
    dct:created "2026-02-04"^^xsd:date ;
    rdfs:isDefinedBy sector-health-owl: ;
    rdfs:subClassOf sector-health-owl:TrainTestAndEvaluateHealthAlgorithms ;
    sw:term_status "accepted"@en ;
    skos:definition "Purposes associated with training, testing and evaluating algorithms in digital health applications"@en ;
    skos:prefLabel "Train, Test and Evaluate Health Apps Algorithms"@en .

sector-health-owl:TrainTestAndEvaluateMedicalDevicesAlgorithms a rdfs:Class,
        owl:Class,
        dpv-owl:Purpose ;
    dct:contributor _:person-beatriz-esteves ;
    dct:created "2026-02-04"^^xsd:date ;
    rdfs:isDefinedBy sector-health-owl: ;
    rdfs:subClassOf sector-health-owl:TrainTestAndEvaluateHealthAlgorithms ;
    sw:term_status "accepted"@en ;
    skos:definition "Purposes associated with training, testing and evaluating algorithms in medical devices"@en ;
    skos:prefLabel "Train, Test and Evaluate Medical Devices Algorithms"@en .

sector-health-owl:TranscriptomicData a rdfs:Class,
        owl:Class,
        dpv-owl:PersonalData ;
    dct:contributor _:person-beatriz-esteves ;
    dct:created "2026-02-04"^^xsd:date ;
    rdfs:isDefinedBy sector-health-owl: ;
    rdfs:subClassOf pd-owl:Molecular ;
    sw:term_status "accepted"@en ;
    skos:definition "Information about transcriptomic data"@en ;
    skos:prefLabel "Transcriptomic Data"@en .

sector-health-owl:TreatmentOptimisation a rdfs:Class,
        owl:Class,
        dpv-owl:Purpose ;
    dct:created "2024-12-01"^^xsd:date ;
    rdfs:isDefinedBy sector-health-owl: ;
    rdfs:subClassOf dpv-owl:ServiceOptimisation,
        sector-health-owl:Optimisation ;
    sw:term_status "accepted"@en ;
    skos:definition "Purposes associated with identifying optimisations related to use of treatments and related processes as part of healthcare services"@en ;
    skos:prefLabel "Treatment Optimisation"@en .

sector-health-owl:VaccinationManagement a rdfs:Class,
        owl:Class,
        dpv-owl:Purpose ;
    dct:created "2024-12-01"^^xsd:date ;
    rdfs:isDefinedBy sector-health-owl: ;
    rdfs:subClassOf sector-health-owl:PreventativeCareManagement ;
    sw:term_status "accepted"@en ;
    skos:definition "Purposes associated with management of vaccinations as part of healthcare services"@en ;
    skos:prefLabel "Vaccination Management"@en .

sector-health-owl:WellnessAppDistributor a rdfs:Class,
        owl:Class,
        tech-owl:Actor ;
    dct:contributor _:person-beatriz-esteves ;
    dct:created "2026-02-04"^^xsd:date ;
    dct:source "EHDS Art.47.9"@en ;
    rdfs:isDefinedBy sector-health-owl: ;
    rdfs:subClassOf tech-owl:Distributor ;
    sw:term_status "accepted"@en ;
    skos:definition "Actor that distributes wellness apps"@en ;
    skos:prefLabel "Wellness App Distributor"@en .

sector-health-owl:WellnessAppManufacturer a rdfs:Class,
        owl:Class,
        tech-owl:Actor ;
    dct:contributor _:person-beatriz-esteves ;
    dct:created "2026-02-04"^^xsd:date ;
    rdfs:isDefinedBy sector-health-owl: ;
    rdfs:subClassOf tech-owl:Manufacturer ;
    sw:term_status "accepted"@en ;
    skos:definition "Actor that manufactures wellness apps"@en ;
    skos:prefLabel "Wellness App Manufacturer"@en .

sector-health-owl:WellnessAppSupplier a rdfs:Class,
        owl:Class,
        tech-owl:Actor ;
    dct:contributor _:person-beatriz-esteves ;
    dct:created "2026-02-04"^^xsd:date ;
    rdfs:isDefinedBy sector-health-owl: ;
    rdfs:subClassOf tech-owl:Supplier ;
    sw:term_status "accepted"@en ;
    skos:definition "Actor that supplies wellness apps"@en ;
    skos:prefLabel "Wellness App Supplier"@en .

sector-health-owl:WellnessApplication a rdfs:Class,
        owl:Class,
        dpv-owl:Technology ;
    dct:contributor _:person-beatriz-esteves ;
    dct:created "2025-10-28"^^xsd:date ;
    rdfs:isDefinedBy sector-health-owl: ;
    rdfs:subClassOf sector-health-owl:HealthApplication ;
    sw:term_status "accepted"@en ;
    skos:definition "Software component for the processing of electronic health data originating from wellness applications"@en ;
    skos:prefLabel "Wellness Application"@en .

sector-health-owl:WellnessData a rdfs:Class,
        owl:Class,
        dpv-owl:PersonalData ;
    dct:contributor _:person-beatriz-esteves ;
    dct:created "2026-02-04"^^xsd:date ;
    rdfs:isDefinedBy sector-health-owl: ;
    rdfs:subClassOf pd-owl:Behavioural ;
    sw:term_status "accepted"@en ;
    skos:definition "Information about wellness"@en ;
    skos:prefLabel "Wellness Data"@en .

sector-health-owl:WorkforceManagement a rdfs:Class,
        owl:Class,
        dpv-owl:Purpose ;
    dct:created "2024-12-01"^^xsd:date ;
    rdfs:isDefinedBy sector-health-owl: ;
    rdfs:subClassOf sector-health-owl:HealthcareManagement ;
    sw:term_status "accepted"@en ;
    skos:definition "Purposes associated with management of workforce involved in provision of healthcare services"@en ;
    skos:prefLabel "Workforce Management"@en .

sector-health-owl:serialisation-html a profile:ResourceDescriptor ;
    dct:conformsTo <https://www.w3.org/TR/html/> ;
    dct:format <https://www.iana.org/assignments/media-types/text/html> ;
    dct:title "Health Sector Concepts - HTML serialisation" ;
    profile:hasArtifact <https://w3id.org/dpv/sector/health/sector-health-owl.html> ;
    profile:hasRole role:specification .

sector-health-owl:serialisation-jsonld a profile:ResourceDescriptor ;
    dct:conformsTo <https://www.w3.org/TR/json-ld11/> ;
    dct:format <https://www.iana.org/assignments/media-types/application/ld+json> ;
    dct:title "Health Sector Concepts - JSON-LD serialisation" ;
    profile:hasArtifact <https://w3id.org/dpv/sector/health/sector-health-owl.jsonld> ;
    profile:hasRole role:vocabulary .

sector-health-owl:serialisation-n3 a profile:ResourceDescriptor ;
    dct:conformsTo <https://www.w3.org/TeamSubmission/n3/> ;
    dct:format <https://www.iana.org/assignments/media-types/text/n3> ;
    dct:title "Health Sector Concepts - N3 serialisation" ;
    profile:hasArtifact <https://w3id.org/dpv/sector/health/sector-health-owl.n3> ;
    profile:hasRole role:vocabulary .

sector-health-owl:serialisation-rdf a profile:ResourceDescriptor ;
    dct:conformsTo rdf: ;
    dct:format <https://www.iana.org/assignments/media-types/application/rdf+xml> ;
    dct:title "Health Sector Concepts - RDF/XML serialisation" ;
    profile:hasArtifact <https://w3id.org/dpv/sector/health/sector-health-owl.rdf> ;
    profile:hasRole role:vocabulary .

sector-health-owl:serialisation-ttl a profile:ResourceDescriptor ;
    dct:conformsTo <https://www.w3.org/TR/turtle/> ;
    dct:format <https://www.iana.org/assignments/media-types/text/turtle> ;
    dct:title "Health Sector Concepts - Turtle serialisation" ;
    profile:hasArtifact <https://w3id.org/dpv/sector/health/sector-health-owl.ttl> ;
    profile:hasRole role:vocabulary .

<https://w3id.org/dpv/examples> a profile:ResourceDescriptor ;
    dct:conformsTo <https://www.w3.org/TR/html/> ;
    dct:format <https://www.iana.org/assignments/media-types/text/html> ;
    dct:title "Examples" ;
    profile:hasArtifact <https://w3id.org/dpv/examples> ;
    profile:hasRole role:guidance .

<https://w3id.org/dpv/guides> a profile:ResourceDescriptor ;
    dct:conformsTo <https://www.w3.org/TR/html/> ;
    dct:format <https://www.iana.org/assignments/media-types/text/html> ;
    dct:title "Guides for Data Privacy Vocabulary" ;
    profile:hasArtifact <https://w3id.org/dpv/guides> ;
    profile:hasRole role:guidance .

<https://w3id.org/dpv/primer> a profile:ResourceDescriptor ;
    dct:conformsTo <https://www.w3.org/TR/html/> ;
    dct:format <https://www.iana.org/assignments/media-types/text/html> ;
    dct:title "Primer for Data Privacy Vocabulary" ;
    profile:hasArtifact <https://w3id.org/dpv/primer> ;
    profile:hasRole role:guidance .

sector-health-owl: a owl:Ontology,
        profile:Profile ;
    dct:bibliographicCitation "Harshvardhan J. Pandit, Beatriz Esteves, Georg P. Krog, Paul Ryan, Delaram Golpayegani, Julian Flake (2025) Data Privacy Vocabulary (DPV)  Version 2.0. In: Demartini, G., et al. The Semantic Web  ISWC 2024. ISWC 2024. Lecture Notes in Computer Science, vol 15233. Springer, Cham. https://doi.org/10.1007/978-3-031-77847-6_10" ;
    dct:conformsTo <http://www.w3.org/2002/07/owl>,
        "http://www.w3.org/2000/01/rdf-schema",
        "http://www.w3.org/2004/02/skos/core" ;
    dct:contributor _:person-arthit-suriyawongkul,
        _:person-beatriz-esteves,
        _:person-delaram-golpayegani,
        _:person-georg-p-krog,
        _:person-harshvardhan-j-pandit,
        _:person-julian-flake ;
    dct:created "2024-12-01"@en ;
    dct:creator _:person-beatriz-esteves,
        _:person-harshvardhan-j-pandit,
        _:person-julian-flake ;
    dct:description "Extension to the Data Privacy Vocabulary (DPV) providing concepts for the health sector"@en ;
    dct:hasVersion sector-health-owl: ;
    dct:identifier "https://w3id.org/dpv/sector/health" ;
    dct:issued "2024-12-01"@en ;
    dct:license <https://www.w3.org/copyright/document-license-2023/> ;
    dct:modified "2026-02-25"@en ;
    dct:publisher <https://www.w3.org/> ;
    dct:source <https://www.w3.org/groups/cg/dpvcg/> ;
    dct:title "Health Sector Concepts"@en ;
    bibo:doi "10.5281/zenodo.12505841" ;
    bibo:status "http://purl.org/ontology/bibo/status/draft" ;
    vann:preferredNamespacePrefix "sector-health" ;
    vann:preferredNamespaceUri "https://w3id.org/dpv/sector/health#" ;
    rdfs:Label "SECTOR-HEALTH"@en ;
    owl:versionIRI <https://w3id.org/dpv/2.3/sector/health/owl#> ;
    owl:versionInfo "2.3" ;
    profile:hasResource <https://w3id.org/dpv/examples>,
        <https://w3id.org/dpv/guides>,
        <https://w3id.org/dpv/primer>,
        sector-health-owl:serialisation-html,
        sector-health-owl:serialisation-jsonld,
        sector-health-owl:serialisation-n3,
        sector-health-owl:serialisation-rdf,
        sector-health-owl:serialisation-ttl ;
    profile:isProfileOf <http://www.w3.org/2002/07/owl>,
        <https://w3id.org/dpv/owl>,
        sector-health-owl: ;
    foaf:logo <https://w3id.org/dpv/media/logo.png> ;
    schema:version "2.3" .

_:org-ai-accountability-lab-aial-trinity-college-dublin a foaf:Organization ;
    foaf:name "AI Accountability Lab (AIAL), Trinity College Dublin" .

_:org-idlab-imec-ghent-university a foaf:Organization ;
    foaf:name "IDLab, IMEC, Ghent University" .

_:org-signatu-as a foaf:Organization ;
    foaf:name "Signatu AS" .

_:org-university-of-koblenz a foaf:Organization ;
    foaf:name "University of Koblenz" .

_:org-adapt-centre-trinity-college-dublin a foaf:Organization ;
    foaf:name "ADAPT Centre, Trinity College Dublin" .

_:person-arthit-suriyawongkul a dct:Agent,
        foaf:Person ;
    scoro:hasORCID "0000-0002-9698-1899" ;
    org:memberOf _:org-adapt-centre-trinity-college-dublin ;
    foaf:name "Arthit Suriyawongkul" .

_:person-delaram-golpayegani a dct:Agent,
        foaf:Person ;
    scoro:hasORCID "0000-0002-1208-186X" ;
    org:memberOf _:org-adapt-centre-trinity-college-dublin ;
    foaf:name "Delaram Golpayegani" .

_:person-georg-p-krog a dct:Agent,
        foaf:Person ;
    org:memberOf _:org-signatu-as ;
    foaf:homepage "https://www.linkedin.com/in/georg-philip-krog-a2a278104/" ;
    foaf:name "Georg P. Krog" .

_:person-harshvardhan-j-pandit a dct:Agent,
        foaf:Person ;
    scoro:hasORCID "0000-0002-5068-3714" ;
    org:memberOf _:org-ai-accountability-lab-aial-trinity-college-dublin ;
    foaf:homepage "https://harshp.com/" ;
    foaf:name "Harshvardhan J. Pandit" .

_:person-julian-flake a dct:Agent,
        foaf:Person ;
    scoro:hasORCID "0009-0006-4623-1463" ;
    org:memberOf _:org-university-of-koblenz ;
    foaf:name "Julian Flake" .

_:person-beatriz-esteves a dct:Agent,
        foaf:Person ;
    scoro:hasORCID "0000-0003-0259-7560" ;
    org:memberOf _:org-idlab-imec-ghent-university ;
    foaf:homepage "https://w3id.org/people/besteves" ;
    foaf:name "Beatriz Esteves" .

