@prefix bibo: <http://purl.org/ontology/bibo/> .
@prefix dct: <http://purl.org/dc/terms/> .
@prefix dpv: <https://w3id.org/dpv#> .
@prefix foaf: <http://xmlns.com/foaf/0.1/> .
@prefix org: <http://www.w3.org/ns/org#> .
@prefix owl: <http://www.w3.org/2002/07/owl#> .
@prefix profile: <http://www.w3.org/ns/dx/prof/> .
@prefix rdf: <http://www.w3.org/1999/02/22-rdf-syntax-ns#> .
@prefix rdfs: <http://www.w3.org/2000/01/rdf-schema#> .
@prefix role: <http://www.w3.org/ns/dx/prof/role/> .
@prefix schema: <https://schema.org/> .
@prefix scoro: <http://purl.org/spar/scoro/> .
@prefix sector-publicservices: <https://w3id.org/dpv/sector/publicservices#> .
@prefix skos: <http://www.w3.org/2004/02/skos/core#> .
@prefix sw: <http://www.w3.org/2003/06/sw-vocab-status/ns#> .
@prefix vann: <http://purl.org/vocab/vann/> .
@prefix xsd: <http://www.w3.org/2001/XMLSchema#> .

sector-publicservices:HousingWelfareManagement a rdfs:Class,
        skos:Concept,
        dpv:Purpose ;
    dct:created "2024-12-01"^^xsd:date ;
    rdfs:isDefinedBy sector-publicservices: ;
    sw:term_status "accepted"@en ;
    skos:broader sector-publicservices:SocialAssistanceManagement ;
    skos:definition "Purposes associated with management of housing as part of social assistance and welfare services"@en ;
    skos:inScheme sector-publicservices:purposes-classes ;
    skos:prefLabel "Housing Welfare Management"@en .

sector-publicservices:PublicServiceDistributionManagement a rdfs:Class,
        skos:Concept,
        dpv:Purpose ;
    dct:created "2024-12-01"^^xsd:date ;
    rdfs:isDefinedBy sector-publicservices: ;
    sw:term_status "accepted"@en ;
    skos:broader sector-publicservices:PublicServiceProvision ;
    skos:definition "Purposes associated with managing the distribution in relation to public services, such as increasing, decreasing, granting, revoking, or reducing the service or related benefits"@en ;
    skos:inScheme sector-publicservices:purposes-classes ;
    skos:prefLabel "Public Service Distribution Management"@en .

sector-publicservices:PublicServiceEligibilityAssessment a rdfs:Class,
        skos:Concept,
        dpv:Purpose ;
    dct:created "2024-12-01"^^xsd:date ;
    rdfs:isDefinedBy sector-publicservices: ;
    sw:term_status "accepted"@en ;
    skos:broader sector-publicservices:PublicServiceManagement ;
    skos:definition "Purposes associated with assessing the eligbility of a person to receive or continue to receive public services"@en ;
    skos:inScheme sector-publicservices:purposes-classes ;
    skos:prefLabel "Public Service Eligibility Assessment"@en .

sector-publicservices:PublicServiceFraudPreventionDetection a rdfs:Class,
        skos:Concept,
        dpv:Purpose ;
    dct:created "2024-12-01"^^xsd:date ;
    rdfs:isDefinedBy sector-publicservices: ;
    sw:term_status "accepted"@en ;
    skos:broader dpv:FraudPreventionAndDetection,
        sector-publicservices:PublicServiceManagement ;
    skos:definition "Purposes associated with fraud detection and prevention in relation to public services"@en ;
    skos:inScheme sector-publicservices:purposes-classes ;
    skos:prefLabel "Public Service Fraud Prevention Detection"@en .

sector-publicservices:PublicServiceManagement a rdfs:Class,
        skos:Concept,
        dpv:Purpose ;
    dct:created "2024-12-01"^^xsd:date ;
    rdfs:isDefinedBy sector-publicservices: ;
    sw:term_status "accepted"@en ;
    skos:broader dpv:PublicBenefit ;
    skos:definition "Purposes associated with management of public services"@en ;
    skos:inScheme sector-publicservices:purposes-classes ;
    skos:prefLabel "Pubilc Service Management"@en .

sector-publicservices:PublicServiceProvision a rdfs:Class,
        skos:Concept,
        dpv:Purpose ;
    dct:created "2024-12-01"^^xsd:date ;
    rdfs:isDefinedBy sector-publicservices: ;
    sw:term_status "accepted"@en ;
    skos:broader dpv:ServiceProvision,
        sector-publicservices:PublicServiceManagement ;
    skos:definition "Purposes associated with provision of public services"@en ;
    skos:inScheme sector-publicservices:purposes-classes ;
    skos:prefLabel "Public Service Provision"@en .

sector-publicservices:SocialAssistanceManagement a rdfs:Class,
        skos:Concept,
        dpv:Purpose ;
    dct:created "2024-12-01"^^xsd:date ;
    rdfs:isDefinedBy sector-publicservices: ;
    sw:term_status "accepted"@en ;
    skos:broader sector-publicservices:SocialWelfareManagement ;
    skos:definition "Purposes associated with management of social assistance services"@en ;
    skos:inScheme sector-publicservices:purposes-classes ;
    skos:prefLabel "Social Assistance Management"@en .

sector-publicservices:SocialInsuranceManagement a rdfs:Class,
        skos:Concept,
        dpv:Purpose ;
    dct:created "2024-12-01"^^xsd:date ;
    rdfs:isDefinedBy sector-publicservices: ;
    sw:term_status "accepted"@en ;
    skos:broader sector-publicservices:SocialAssistanceManagement ;
    skos:definition "Purposes associated with management of social insurance as part of social assistance and welfare services"@en ;
    skos:inScheme sector-publicservices:purposes-classes ;
    skos:prefLabel "Social Insurance Management"@en .

sector-publicservices:SocialSecurityManagement a rdfs:Class,
        skos:Concept,
        dpv:Purpose ;
    dct:created "2024-12-01"^^xsd:date ;
    rdfs:isDefinedBy sector-publicservices: ;
    sw:term_status "accepted"@en ;
    skos:broader sector-publicservices:SocialAssistanceManagement ;
    skos:definition "Purposes associated with management of social security as part of social assistance and welfare services"@en ;
    skos:inScheme sector-publicservices:purposes-classes ;
    skos:prefLabel "Social Security Management"@en .

sector-publicservices:SocialWelfareDistributionManagement a rdfs:Class,
        skos:Concept,
        dpv:Purpose ;
    dct:created "2024-12-01"^^xsd:date ;
    rdfs:isDefinedBy sector-publicservices: ;
    sw:term_status "accepted"@en ;
    skos:broader sector-publicservices:SocialWelfareProvision ;
    skos:definition "Purposes associated with managing the distribution in relation to social welfare, such as increasing, decreasing, granting, revoking, or reducing the service or related benefits"@en ;
    skos:inScheme sector-publicservices:purposes-classes ;
    skos:prefLabel "Social Welfare Distribution Management"@en .

sector-publicservices:SocialWelfareEligibilityAssessment a rdfs:Class,
        skos:Concept,
        dpv:Purpose ;
    dct:created "2024-12-01"^^xsd:date ;
    rdfs:isDefinedBy sector-publicservices: ;
    sw:term_status "accepted"@en ;
    skos:broader sector-publicservices:SocialWelfareManagement ;
    skos:definition "Purposes associated with assessment of eligibility of a person to receive or continue to receive social welfare"@en ;
    skos:inScheme sector-publicservices:purposes-classes ;
    skos:prefLabel "Social Welfare Eligibility Assessment"@en .

sector-publicservices:SocialWelfareEnrollmentManagement a rdfs:Class,
        skos:Concept,
        dpv:Purpose ;
    dct:created "2024-12-01"^^xsd:date ;
    rdfs:isDefinedBy sector-publicservices: ;
    sw:term_status "accepted"@en ;
    skos:broader sector-publicservices:SocialWelfareManagement ;
    skos:definition "Purposes associated with enrollment and managing enrollment of persons for the purposes of providing social welfare"@en ;
    skos:inScheme sector-publicservices:purposes-classes ;
    skos:prefLabel "Social Welfare Enrollment Management"@en .

sector-publicservices:SocialWelfareManagement a rdfs:Class,
        skos:Concept,
        dpv:Purpose ;
    dct:created "2024-12-01"^^xsd:date ;
    rdfs:isDefinedBy sector-publicservices: ;
    sw:term_status "accepted"@en ;
    skos:broader sector-publicservices:PublicServiceManagement ;
    skos:definition "Purposes associated with management of social welfare"@en ;
    skos:inScheme sector-publicservices:purposes-classes ;
    skos:prefLabel "Social Welfare Management"@en .

sector-publicservices:SocialWelfareProvision a rdfs:Class,
        skos:Concept,
        dpv:Purpose ;
    dct:created "2024-12-01"^^xsd:date ;
    rdfs:isDefinedBy sector-publicservices: ;
    sw:term_status "accepted"@en ;
    skos:broader sector-publicservices:PublicServiceProvision,
        sector-publicservices:SocialWelfareManagement ;
    skos:definition "Purposes associated with provision of social welfare"@en ;
    skos:inScheme sector-publicservices:purposes-classes ;
    skos:prefLabel "Social Welfare Provision"@en .

sector-publicservices:SocialWelfareRiskAssessment a rdfs:Class,
        skos:Concept,
        dpv:Purpose ;
    dct:created "2024-12-01"^^xsd:date ;
    rdfs:isDefinedBy sector-publicservices: ;
    sw:term_status "accepted"@en ;
    skos:broader dpv:FraudPreventionAndDetection,
        dpv:OrganisationRiskManagement,
        sector-publicservices:SocialWelfareManagement ;
    skos:definition "Purposes associated with conducting risk and impact assessments in relation to use of social welfare"@en ;
    skos:inScheme sector-publicservices:purposes-classes ;
    skos:prefLabel "Social Welfare Risk Assessment"@en .

<https://w3id.org/dpv/sector/publicservices> a owl:Ontology,
        profile:Profile ;
    dct:bibliographicCitation "Harshvardhan J. Pandit, Beatriz Esteves, Georg P. Krog, Paul Ryan, Delaram Golpayegani, Julian Flake (2025) Data Privacy Vocabulary (DPV) – Version 2.0. In: Demartini, G., et al. The Semantic Web – ISWC 2024. ISWC 2024. Lecture Notes in Computer Science, vol 15233. Springer, Cham. https://doi.org/10.1007/978-3-031-77847-6_10" ;
    dct:conformsTo "http://www.w3.org/2000/01/rdf-schema",
        "http://www.w3.org/2004/02/skos/core" ;
    dct:created "2024-12-01"@en ;
    dct:creator [ a dct:Agent,
                foaf:Person ;
            scoro:hasORCID "0000-0002-5068-3714" ;
            org:memberOf [ a foaf:Organization ;
                    foaf:name "ADAPT Centre, Dublin City University" ] ;
            foaf:homepage "https://harshp.com/" ;
            foaf:name "Harshvardhan J. Pandit" ] ;
    dct:description "Extension to the Data Privacy Vocabulary (DPV) providing concepts for the public services sector"@en ;
    dct:identifier "https://w3id.org/dpv/sector/publicservices" ;
    dct:issued "2024-12-01"@en ;
    dct:license <https://www.w3.org/copyright/document-license-2023/> ;
    dct:modified "2025-03-16"@en ;
    dct:publisher <https://www.w3.org/> ;
    dct:source <https://www.w3.org/groups/cg/dpvcg/> ;
    dct:title "Public Services Sector Concepts"@en ;
    bibo:doi "10.5281/zenodo.12505841" ;
    bibo:status "http://purl.org/ontology/bibo/status/draft" ;
    vann:preferredNamespacePrefix "sector-publicservices" ;
    vann:preferredNamespaceUri "https://w3id.org/dpv/sector/publicservices#" ;
    rdfs:Label "SECTOR-PUBLICSERVICES"@en ;
    owl:versionIRI <https://w3id.org/dpv/2.1/sector/publicservices> ;
    owl:versionInfo "2.1" ;
    profile:hasResource <https://w3id.org/dpv/examples>,
        <https://w3id.org/dpv/guides>,
        <https://w3id.org/dpv/primer>,
        sector-publicservices:serialisation-html,
        sector-publicservices:serialisation-jsonld,
        sector-publicservices:serialisation-n3,
        sector-publicservices:serialisation-rdf,
        sector-publicservices:serialisation-ttl ;
    profile:isProfileOf rdfs:,
        skos:,
        <https://w3id.org/dpv> ;
    foaf:logo <https://w3id.org/dpv/media/logo.png> ;
    schema:version "2.1" .

sector-publicservices:serialisation-html a profile:ResourceDescriptor ;
    dct:conformsTo <https://www.w3.org/TR/html/> ;
    dct:format <https://www.iana.org/assignments/media-types/text/html> ;
    dct:title "Public Services Sector Concepts - HTML serialiation" ;
    profile:hasArtifact <https://w3id.org/dpv/sector/publicservices/sector-publicservices.html> ;
    profile:hasRole role:specification .

sector-publicservices:serialisation-jsonld a profile:ResourceDescriptor ;
    dct:conformsTo <https://www.w3.org/TR/json-ld11/> ;
    dct:format <https://www.iana.org/assignments/media-types/application/ld+json> ;
    dct:title "Public Services Sector Concepts - JSON-LD serialiation" ;
    profile:hasArtifact <https://w3id.org/dpv/sector/publicservices/sector-publicservices.jsonld> ;
    profile:hasRole role:vocabulary .

sector-publicservices:serialisation-n3 a profile:ResourceDescriptor ;
    dct:conformsTo <https://www.w3.org/TeamSubmission/n3/> ;
    dct:format <https://www.iana.org/assignments/media-types/text/n3> ;
    dct:title "Public Services Sector Concepts - N3 serialiation" ;
    profile:hasArtifact <https://w3id.org/dpv/sector/publicservices/sector-publicservices.n3> ;
    profile:hasRole role:vocabulary .

sector-publicservices:serialisation-rdf a profile:ResourceDescriptor ;
    dct:conformsTo rdf: ;
    dct:format <https://www.iana.org/assignments/media-types/application/rdf+xml> ;
    dct:title "Public Services Sector Concepts - RDF/XML serialiation" ;
    profile:hasArtifact <https://w3id.org/dpv/sector/publicservices/sector-publicservices.rdf> ;
    profile:hasRole role:vocabulary .

sector-publicservices:serialisation-ttl a profile:ResourceDescriptor ;
    dct:conformsTo <https://www.w3.org/TR/turtle/> ;
    dct:format <https://www.iana.org/assignments/media-types/text/turtle> ;
    dct:title "Public Services Sector Concepts - Turtle serialiation" ;
    profile:hasArtifact <https://w3id.org/dpv/sector/publicservices/sector-publicservices.ttl> ;
    profile:hasRole role:vocabulary .

<https://w3id.org/dpv/examples> a profile:ResourceDescriptor ;
    dct:conformsTo <https://www.w3.org/TR/html/> ;
    dct:format <https://www.iana.org/assignments/media-types/text/html> ;
    dct:title "Examples for Data Privacy Vocabulary" ;
    profile:hasArtifact <https://w3id.org/dpv/examples> ;
    profile:hasRole role:guidance .

<https://w3id.org/dpv/guides> a profile:ResourceDescriptor ;
    dct:conformsTo <https://www.w3.org/TR/html/> ;
    dct:format <https://www.iana.org/assignments/media-types/text/html> ;
    dct:title "Guides for Data Privacy Vocabulary" ;
    profile:hasArtifact <https://w3id.org/dpv/guides> ;
    profile:hasRole role:guidance .

<https://w3id.org/dpv/primer> a profile:ResourceDescriptor ;
    dct:conformsTo <https://www.w3.org/TR/html/> ;
    dct:format <https://www.iana.org/assignments/media-types/text/html> ;
    dct:title "Primer for Data Privacy Vocabulary" ;
    profile:hasArtifact <https://w3id.org/dpv/primer> ;
    profile:hasRole role:guidance .

sector-publicservices:purposes-classes a skos:ConceptScheme .

