@prefix bibo: <http://purl.org/ontology/bibo/> .
@prefix dcam: <http://purl.org/dc/dcam/> .
@prefix dct: <http://purl.org/dc/terms/> .
@prefix dpv-owl: <https://w3id.org/dpv/owl#> .
@prefix foaf: <http://xmlns.com/foaf/0.1/> .
@prefix ieee-7012-owl: <https://w3id.org/dpv/standards/ieee/7012/owl#> .
@prefix org: <http://www.w3.org/ns/org#> .
@prefix owl: <http://www.w3.org/2002/07/owl#> .
@prefix profile: <http://www.w3.org/ns/dx/prof/> .
@prefix rdf: <http://www.w3.org/1999/02/22-rdf-syntax-ns#> .
@prefix rdfs: <http://www.w3.org/2000/01/rdf-schema#> .
@prefix role: <http://www.w3.org/ns/dx/prof/role/> .
@prefix schema: <https://schema.org/> .
@prefix scoro: <http://purl.org/spar/scoro/> .
@prefix skos: <http://www.w3.org/2004/02/skos/core#> .
@prefix sw: <http://www.w3.org/2003/06/sw-vocab-status/ns#> .
@prefix vann: <http://purl.org/vocab/vann/> .
@prefix xsd: <http://www.w3.org/2001/XMLSchema#> .

ieee-7012-owl:Agent a rdfs:Class,
        owl:Class ;
    dct:created "2024-12-17"^^xsd:date ;
    rdfs:isDefinedBy ieee-7012-owl: ;
    rdfs:subClassOf dpv-owl:Entity ;
    sw:term_status "accepted"@en ;
    skos:definition "An Agent is any software or a combination of software and hardware that works exclusively for its party, and which may be provided by a third party but must be controlled and be responsible to the party it represents"@en ;
    skos:prefLabel "Agent"@en .

ieee-7012-owl:AgentAllowsNegotiation a rdfs:Class,
        owl:Class,
        ieee-7012-owl:AgentNegotiationBehaviour ;
    dct:created "2024-12-17"^^xsd:date ;
    rdfs:isDefinedBy ieee-7012-owl: ;
    rdfs:subClassOf ieee-7012-owl:AgentNegotiationBehaviour ;
    sw:term_status "accepted"@en ;
    skos:definition "Term that indicates the Agent should allow negotiations"@en ;
    skos:prefLabel "Agent Allows Negotiation"@en .

ieee-7012-owl:AgentAllowsNegotiationOnlyKnownParty a rdfs:Class,
        owl:Class,
        ieee-7012-owl:AgentNegotiationBehaviour ;
    dct:created "2024-12-17"^^xsd:date ;
    rdfs:isDefinedBy ieee-7012-owl: ;
    rdfs:subClassOf ieee-7012-owl:AgentAllowsNegotiation ;
    sw:term_status "accepted"@en ;
    skos:definition "Term that indicates the Agent should allow negotiations but only from known parties"@en ;
    skos:prefLabel "Agent Allows Negotiation Only Known Party"@en .

ieee-7012-owl:AgentAllowsNegotiationOnlyPriorAgreementParty a rdfs:Class,
        owl:Class,
        ieee-7012-owl:AgentNegotiationBehaviour ;
    dct:created "2024-12-17"^^xsd:date ;
    rdfs:isDefinedBy ieee-7012-owl: ;
    rdfs:subClassOf ieee-7012-owl:AgentAllowsNegotiationOnlyKnownParty ;
    sw:term_status "accepted"@en ;
    skos:definition "Term that indicates the Agent should allow negotiations but only from known parties with whom an agreement was established in the past"@en ;
    skos:prefLabel "Agent Allows Negotiation Only Prior Agreement Party"@en .

ieee-7012-owl:AgentAllowsRequests a rdfs:Class,
        owl:Class,
        ieee-7012-owl:AgentRequestBehaviour ;
    dct:created "2024-12-17"^^xsd:date ;
    rdfs:isDefinedBy ieee-7012-owl: ;
    rdfs:subClassOf ieee-7012-owl:AgentRequestBehaviour ;
    sw:term_status "accepted"@en ;
    skos:definition "Term that indicates the Agent should allow requests to be made"@en ;
    skos:prefLabel "Agent Allows Requests"@en .

ieee-7012-owl:AgentAllowsRequestsOnlyKnownParty a rdfs:Class,
        owl:Class,
        ieee-7012-owl:AgentRequestBehaviour ;
    dct:created "2024-12-17"^^xsd:date ;
    rdfs:isDefinedBy ieee-7012-owl: ;
    rdfs:subClassOf ieee-7012-owl:AgentAllowsRequests ;
    sw:term_status "accepted"@en ;
    skos:definition "Term that indicates the Agent should allow requests to be made but only from prior known parties"@en ;
    skos:prefLabel "Agent Allows Requests Only Known Party"@en .

ieee-7012-owl:AgentAllowsRequestsOnlyPriorAgreementParty a rdfs:Class,
        owl:Class,
        ieee-7012-owl:AgentRequestBehaviour ;
    dct:created "2024-12-17"^^xsd:date ;
    rdfs:isDefinedBy ieee-7012-owl: ;
    rdfs:subClassOf ieee-7012-owl:AgentAllowsRequestsOnlyKnownParty ;
    sw:term_status "accepted"@en ;
    skos:definition "Term that indicates the Agent should allow requests to be made but only from prior known parties with whom an agreement was established in the past"@en ;
    skos:prefLabel "Agent Allows Requests Only Prior Agreement Party"@en .

ieee-7012-owl:AgentBehaviour a rdfs:Class,
        owl:Class ;
    dct:created "2024-12-17"^^xsd:date ;
    rdfs:isDefinedBy ieee-7012-owl: ;
    rdfs:subClassOf dpv-owl:ContractualClause ;
    sw:term_status "accepted"@en ;
    skos:definition "Term that indicates the behaviour of the Agent"@en ;
    skos:prefLabel "Agent Behaviour"@en .

ieee-7012-owl:AgentDisallowsNegotiation a rdfs:Class,
        owl:Class,
        ieee-7012-owl:AgentNegotiationBehaviour ;
    dct:created "2024-12-17"^^xsd:date ;
    rdfs:isDefinedBy ieee-7012-owl: ;
    rdfs:subClassOf ieee-7012-owl:AgentNegotiationBehaviour ;
    sw:term_status "accepted"@en ;
    skos:definition "Term that indicates the Agent should not allow any negotiations"@en ;
    skos:prefLabel "Agent Disallows Negotiation"@en .

ieee-7012-owl:AgentDisallowsRequests a rdfs:Class,
        owl:Class,
        ieee-7012-owl:AgentRequestBehaviour ;
    dct:created "2024-12-17"^^xsd:date ;
    rdfs:isDefinedBy ieee-7012-owl: ;
    rdfs:subClassOf ieee-7012-owl:AgentRequestBehaviour ;
    sw:term_status "accepted"@en ;
    skos:definition "Term that indicates the Agent should not allow any requests to be made"@en ;
    skos:prefLabel "Agent Disallows Requests"@en .

ieee-7012-owl:AgentNegotiationBehaviour a rdfs:Class,
        owl:Class ;
    dct:created "2024-12-17"^^xsd:date ;
    rdfs:isDefinedBy ieee-7012-owl: ;
    rdfs:subClassOf ieee-7012-owl:AgentBehaviour ;
    sw:term_status "accepted"@en ;
    skos:definition "Term that indicates the behaviour of the Agent in relation to negotiations"@en ;
    skos:prefLabel "Agent Negotiation Behaviour"@en .

ieee-7012-owl:AgentRequestBehaviour a rdfs:Class,
        owl:Class ;
    dct:created "2024-12-17"^^xsd:date ;
    rdfs:isDefinedBy ieee-7012-owl: ;
    rdfs:subClassOf ieee-7012-owl:AgentBehaviour ;
    sw:term_status "accepted"@en ;
    skos:definition "Term that indicates the behaviour of the Agent in relation to requests"@en ;
    skos:prefLabel "Agent Request Behaviour"@en .

ieee-7012-owl:Agreement a rdfs:Class,
        owl:Class ;
    dct:created "2024-12-17"^^xsd:date ;
    rdfs:isDefinedBy ieee-7012-owl: ;
    rdfs:subClassOf dpv-owl:ContractualClause ;
    sw:term_status "accepted"@en ;
    skos:definition "A compound set of terms or clauses, proposed and offered before a formal contract between parties, and also referred to as a \"proposal\" pr \"proposed agreement\""@en ;
    skos:prefLabel "Agreement"@en .

ieee-7012-owl:AgreementAccepted a rdfs:Class,
        owl:Class,
        ieee-7012-owl:AgreementNegotiationStatus ;
    dct:created "2024-12-17"^^xsd:date ;
    rdfs:isDefinedBy ieee-7012-owl: ;
    rdfs:subClassOf ieee-7012-owl:AgreementNegotiationStatus ;
    sw:term_status "accepted"@en ;
    skos:definition "Status indicating the Agreement Negotiation is completed and the parties have accepted the relevant terms"@en ;
    skos:prefLabel "Agreement Accepted"@en .

ieee-7012-owl:AgreementInteractionRecord a rdfs:Class,
        owl:Class ;
    dct:created "2024-12-17"^^xsd:date ;
    rdfs:isDefinedBy ieee-7012-owl: ;
    rdfs:subClassOf dpv-owl:RecordsOfActivities ;
    sw:term_status "accepted"@en ;
    skos:definition "A record of a interactions conducted in the course of establishing and negotiating agreements, including failed attempts, creation of contracts, and subsequent interactions"@en ;
    skos:prefLabel "Agreement Interaction Record"@en .

ieee-7012-owl:AgreementNegotiation a rdfs:Class,
        owl:Class ;
    dct:created "2024-12-17"^^xsd:date ;
    rdfs:isDefinedBy ieee-7012-owl: ;
    rdfs:subClassOf dpv-owl:Process ;
    sw:term_status "accepted"@en ;
    skos:definition "A negotiation between parties regarding an agreement"@en ;
    skos:prefLabel "Agreement Negotiation"@en .

ieee-7012-owl:AgreementNegotiationClarificationRequired a rdfs:Class,
        owl:Class,
        ieee-7012-owl:AgreementNegotiationStatus ;
    dct:created "2024-12-17"^^xsd:date ;
    rdfs:isDefinedBy ieee-7012-owl: ;
    rdfs:subClassOf ieee-7012-owl:AgreementNegotiationStatus ;
    sw:term_status "accepted"@en ;
    skos:definition "Status indicating the Agreement Negotiation requires a clarification from the other party regarding the relevant context"@en ;
    skos:prefLabel "Agreement Negotiation Clarification Required"@en .

ieee-7012-owl:AgreementNegotiationConfirmationRequired a rdfs:Class,
        owl:Class,
        ieee-7012-owl:AgreementNegotiationStatus ;
    dct:created "2024-12-17"^^xsd:date ;
    rdfs:isDefinedBy ieee-7012-owl: ;
    rdfs:subClassOf ieee-7012-owl:AgreementNegotiationStatus ;
    sw:term_status "accepted"@en ;
    skos:definition "Status indicating the Agreement Negotiation requires a confirmation by a human before it can proceed"@en ;
    skos:prefLabel "Agreement Negotiation Confirmation Required"@en .

ieee-7012-owl:AgreementNegotiationCounterOfferMade a rdfs:Class,
        owl:Class,
        ieee-7012-owl:AgreementNegotiationStatus ;
    dct:created "2024-12-17"^^xsd:date ;
    rdfs:isDefinedBy ieee-7012-owl: ;
    rdfs:subClassOf ieee-7012-owl:AgreementNegotiationStatus ;
    sw:term_status "accepted"@en ;
    skos:definition "Status indicating the terms involved in Agreement Negotiation were not accepted and a counter-offer has been made with a different set of terms"@en ;
    skos:prefLabel "Agreement Negotiation Counter Offer Made"@en .

ieee-7012-owl:AgreementNegotiationExpired a rdfs:Class,
        owl:Class,
        ieee-7012-owl:AgreementNegotiationStatus ;
    dct:created "2024-12-17"^^xsd:date ;
    rdfs:isDefinedBy ieee-7012-owl: ;
    rdfs:subClassOf ieee-7012-owl:AgreementNegotiationStatus ;
    sw:term_status "accepted"@en ;
    skos:definition "Status indicating the Agreement Negotiation has expired due to inactivity by a party or due to other reasons"@en ;
    skos:prefLabel "Agreement Negotiation Expired"@en .

ieee-7012-owl:AgreementNegotiationInitiated a rdfs:Class,
        owl:Class,
        ieee-7012-owl:AgreementNegotiationStatus ;
    dct:created "2024-12-17"^^xsd:date ;
    rdfs:isDefinedBy ieee-7012-owl: ;
    rdfs:subClassOf ieee-7012-owl:AgreementNegotiationStatus ;
    sw:term_status "accepted"@en ;
    skos:definition "Status indicating the Agreement Negotiation process has been initiated"@en ;
    skos:prefLabel "Agreement Negotiation Initiated"@en .

ieee-7012-owl:AgreementNegotiationInvalid a rdfs:Class,
        owl:Class,
        ieee-7012-owl:AgreementNegotiationStatus ;
    dct:created "2024-12-17"^^xsd:date ;
    rdfs:isDefinedBy ieee-7012-owl: ;
    rdfs:subClassOf ieee-7012-owl:AgreementNegotiationStatus ;
    sw:term_status "accepted"@en ;
    skos:definition "Status indicating the Agreement Negotiation is deemed to be invalid and therefore cannot continue"@en ;
    skos:prefLabel "Agreement Negotiation Invalid"@en .

ieee-7012-owl:AgreementNegotiationPaused a rdfs:Class,
        owl:Class,
        ieee-7012-owl:AgreementNegotiationStatus ;
    dct:created "2024-12-17"^^xsd:date ;
    rdfs:isDefinedBy ieee-7012-owl: ;
    rdfs:subClassOf ieee-7012-owl:AgreementNegotiationStatus ;
    sw:term_status "accepted"@en ;
    skos:definition "Status indicating the Agreement Negotiation has been paused i.e. halted or put on hold without a specific decision"@en ;
    skos:prefLabel "Agreement Negotiation Paused"@en .

ieee-7012-owl:AgreementNegotiationPendingResponse a rdfs:Class,
        owl:Class,
        ieee-7012-owl:AgreementNegotiationStatus ;
    dct:created "2024-12-17"^^xsd:date ;
    rdfs:isDefinedBy ieee-7012-owl: ;
    rdfs:subClassOf ieee-7012-owl:AgreementNegotiationStatus ;
    sw:term_status "accepted"@en ;
    skos:definition "Status indicating the Agreement Negotiation process is underway and is awaiting a response from the other party"@en ;
    skos:prefLabel "Agreement Negotiation Pending Response"@en .

ieee-7012-owl:AgreementNegotiationRefused a rdfs:Class,
        owl:Class,
        ieee-7012-owl:AgreementNegotiationStatus ;
    dct:created "2024-12-17"^^xsd:date ;
    rdfs:isDefinedBy ieee-7012-owl: ;
    rdfs:subClassOf ieee-7012-owl:AgreementNegotiationStatus ;
    sw:term_status "accepted"@en ;
    skos:definition "Status indicating the Agreement Negotiation has been refused to be initiated or continued"@en ;
    skos:prefLabel "Agreement Negotiation Refused"@en .

ieee-7012-owl:AgreementNegotiationRequest a rdfs:Class,
        owl:Class ;
    dct:created "2024-12-17"^^xsd:date ;
    rdfs:isDefinedBy ieee-7012-owl: ;
    rdfs:subClassOf dpv-owl:Process ;
    sw:term_status "accepted"@en ;
    skos:definition "A request to initiate negotiation with the goal of finding an acceptable agreement"@en ;
    skos:prefLabel "Agreement Negotiation Request"@en .

ieee-7012-owl:AgreementNegotiationRequested a rdfs:Class,
        owl:Class,
        ieee-7012-owl:AgreementNegotiationStatus ;
    dct:created "2024-12-17"^^xsd:date ;
    rdfs:isDefinedBy ieee-7012-owl: ;
    rdfs:subClassOf ieee-7012-owl:AgreementNegotiationStatus ;
    sw:term_status "accepted"@en ;
    skos:definition "Status indicating the Agreement Negotiation has been requested to be initiated"@en ;
    skos:prefLabel "Agreement Negotiation Requested"@en .

ieee-7012-owl:AgreementNegotiationStatus a rdfs:Class,
        owl:Class ;
    dct:created "2024-12-17"^^xsd:date ;
    rdfs:isDefinedBy ieee-7012-owl: ;
    rdfs:subClassOf dpv-owl:Status ;
    sw:term_status "accepted"@en ;
    skos:definition "Status associated with the Agreement Negotiation"@en ;
    skos:prefLabel "Agreement Negotiation Status"@en .

ieee-7012-owl:AgreementNegotiationTerminated a rdfs:Class,
        owl:Class,
        ieee-7012-owl:AgreementNegotiationStatus ;
    dct:created "2024-12-17"^^xsd:date ;
    rdfs:isDefinedBy ieee-7012-owl: ;
    rdfs:subClassOf ieee-7012-owl:AgreementNegotiationStatus ;
    sw:term_status "accepted"@en ;
    skos:definition "Status indicating the Agreement Negotiation has been terminated by one or more parties"@en ;
    skos:prefLabel "Agreement Negotiation Terminated"@en .

ieee-7012-owl:AgreementNegotiationUnknown a rdfs:Class,
        owl:Class,
        ieee-7012-owl:AgreementNegotiationStatus ;
    dct:created "2024-12-17"^^xsd:date ;
    rdfs:isDefinedBy ieee-7012-owl: ;
    rdfs:subClassOf ieee-7012-owl:AgreementNegotiationStatus ;
    sw:term_status "accepted"@en ;
    skos:definition "Status indicating the state of Agreement Negotiation is unknown"@en ;
    skos:prefLabel "Agreement Negotiation Unknown"@en .

ieee-7012-owl:AgreementPreference a rdfs:Class,
        owl:Class ;
    dct:created "2024-12-17"^^xsd:date ;
    rdfs:isDefinedBy ieee-7012-owl: ;
    rdfs:subClassOf dpv-owl:Rule ;
    sw:term_status "accepted"@en ;
    skos:definition "A preference regarding agreements, such as to indicate which terms are acceptable or unacceptable"@en ;
    skos:prefLabel "Agreement Preference"@en .

ieee-7012-owl:AgreementRefused a rdfs:Class,
        owl:Class,
        ieee-7012-owl:AgreementNegotiationStatus ;
    dct:created "2024-12-17"^^xsd:date ;
    rdfs:isDefinedBy ieee-7012-owl: ;
    rdfs:subClassOf ieee-7012-owl:AgreementNegotiationStatus ;
    sw:term_status "accepted"@en ;
    skos:definition "Status indicating the Agreement Negotiation is completed and the parties have refused the relevant terms"@en ;
    skos:prefLabel "Agreement Refused"@en .

ieee-7012-owl:AgreementRegistry a rdfs:Class,
        owl:Class ;
    dct:created "2024-12-17"^^xsd:date ;
    rdfs:isDefinedBy ieee-7012-owl: ;
    sw:term_status "accepted"@en ;
    skos:definition "A registry hosting agreements that acts as a common repository for parties to utilise as a reference within requests and for negotiating acceptable terms"@en ;
    skos:prefLabel "Agreement Term Registry"@en .

ieee-7012-owl:ConflictResolutionTerm a rdfs:Class,
        owl:Class ;
    dct:created "2024-12-17"^^xsd:date ;
    rdfs:isDefinedBy ieee-7012-owl: ;
    rdfs:subClassOf dpv-owl:ContractualClause ;
    sw:term_status "accepted"@en ;
    skos:definition "Term related to resolving conflicts in Term(s)"@en ;
    skos:prefLabel "Conflict Resolution Term"@en .

ieee-7012-owl:DataDeletionNotRequired a rdfs:Class,
        owl:Class,
        ieee-7012-owl:DataDeletionTerm ;
    dct:created "2025-04-09"^^xsd:date ;
    rdfs:isDefinedBy ieee-7012-owl: ;
    rdfs:subClassOf ieee-7012-owl:DataDeletionTerm ;
    sw:term_status "accepted"@en ;
    skos:definition "Term that indicates deletion of data is not required as an obligation"@en ;
    skos:prefLabel "Data Deletion Not Required"@en .

ieee-7012-owl:DataDeletionOnRequest a rdfs:Class,
        owl:Class,
        dpv-owl:Obligation,
        ieee-7012-owl:DataDeletionTerm ;
    dct:created "2025-04-09"^^xsd:date ;
    rdfs:isDefinedBy ieee-7012-owl: ;
    rdfs:subClassOf dpv-owl:Obligation,
        ieee-7012-owl:DataDeletionTerm ;
    sw:term_status "accepted"@en ;
    skos:definition "Term that indicates deletion of data is required upon request"@en ;
    skos:prefLabel "Data Deletion on Request"@en .

ieee-7012-owl:DataDeletionRequired a rdfs:Class,
        owl:Class,
        dpv-owl:Obligation,
        ieee-7012-owl:DataDeletionTerm ;
    dct:created "2025-04-09"^^xsd:date ;
    rdfs:isDefinedBy ieee-7012-owl: ;
    rdfs:subClassOf dpv-owl:Obligation,
        ieee-7012-owl:DataDeletionTerm ;
    sw:term_status "accepted"@en ;
    skos:definition "Term that indicates deletion of data is required after all associated (approved) processing is completed"@en ;
    skos:prefLabel "Data Deletion Required"@en .

ieee-7012-owl:DataDeletionTerm a rdfs:Class,
        owl:Class ;
    dct:created "2025-04-09"^^xsd:date ;
    rdfs:isDefinedBy ieee-7012-owl: ;
    rdfs:subClassOf dpv-owl:ContractualClause ;
    sw:term_status "accepted"@en ;
    skos:definition "Term that indicates deletion regarding data as an obligation"@en ;
    skos:prefLabel "Data Deletion Term"@en .

ieee-7012-owl:DataSharingTerm a rdfs:Class,
        owl:Class ;
    dct:created "2024-12-17"^^xsd:date ;
    rdfs:isDefinedBy ieee-7012-owl: ;
    rdfs:subClassOf dpv-owl:ContractualClause ;
    sw:term_status "accepted"@en ;
    skos:definition "Term related to Data Sharing"@en ;
    skos:prefLabel "Data Sharing Term"@en .

ieee-7012-owl:DataTransparencyExAnte a rdfs:Class,
        owl:Class,
        dpv-owl:Obligation,
        ieee-7012-owl:DataTransparencyTerm ;
    dct:created "2024-12-17"^^xsd:date ;
    rdfs:isDefinedBy ieee-7012-owl: ;
    rdfs:subClassOf ieee-7012-owl:DataTransparencyRequired ;
    sw:term_status "accepted"@en ;
    skos:definition "Term that indicates transparency regarding data involved and its source is obligated ahead of intended process i.e. ex-ante transparency regarding data involved and its source"@en ;
    skos:prefLabel "Data Transparency Ex Ante"@en .

ieee-7012-owl:DataTransparencyExPost a rdfs:Class,
        owl:Class,
        dpv-owl:Obligation,
        ieee-7012-owl:DataTransparencyTerm ;
    dct:created "2024-12-17"^^xsd:date ;
    rdfs:isDefinedBy ieee-7012-owl: ;
    rdfs:subClassOf ieee-7012-owl:DataTransparencyRequired ;
    sw:term_status "accepted"@en ;
    skos:definition "Term that indicates transparency regarding data involved and its source is obligated after intended process i.e. ex-post transparency regarding data involved and its source"@en ;
    skos:prefLabel "Data Transparency Ex Post"@en .

ieee-7012-owl:DataTransparencyNotRequired a rdfs:Class,
        owl:Class,
        ieee-7012-owl:DataTransparencyTerm ;
    dct:created "2024-12-17"^^xsd:date ;
    rdfs:isDefinedBy ieee-7012-owl: ;
    rdfs:subClassOf ieee-7012-owl:DataTransparencyTerm ;
    sw:term_status "accepted"@en ;
    skos:definition "Term that indicates transparency regarding data involved and its source is not required to be provided"@en ;
    skos:prefLabel "Data Transparency Not Required"@en .

ieee-7012-owl:DataTransparencyOnRequest a rdfs:Class,
        owl:Class,
        dpv-owl:Obligation,
        ieee-7012-owl:DataTransparencyTerm ;
    dct:created "2024-12-17"^^xsd:date ;
    rdfs:isDefinedBy ieee-7012-owl: ;
    rdfs:subClassOf ieee-7012-owl:DataTransparencyRequired ;
    sw:term_status "accepted"@en ;
    skos:definition "Term that indicates transparency regarding data involved and its source is obligated upon request"@en ;
    skos:prefLabel "Data Transparency On Request"@en .

ieee-7012-owl:DataTransparencyRequired a rdfs:Class,
        owl:Class,
        dpv-owl:Obligation,
        ieee-7012-owl:DataTransparencyTerm ;
    dct:created "2024-12-17"^^xsd:date ;
    rdfs:isDefinedBy ieee-7012-owl: ;
    rdfs:subClassOf dpv-owl:Obligation,
        ieee-7012-owl:DataTransparencyTerm ;
    sw:term_status "accepted"@en ;
    skos:definition "Term that indicates transparency regarding data involved and its source is obligated"@en ;
    skos:prefLabel "Data Transparency Required"@en .

ieee-7012-owl:DataTransparencyTerm a rdfs:Class,
        owl:Class ;
    dct:created "2024-12-17"^^xsd:date ;
    rdfs:isDefinedBy ieee-7012-owl: ;
    rdfs:subClassOf ieee-7012-owl:TransparencyTerm ;
    sw:term_status "accepted"@en ;
    skos:definition "Term that indicates transparency regarding data involved and its source as an obligation"@en ;
    skos:prefLabel "Data Transparency Term"@en .

ieee-7012-owl:DeonticInterpretationTerm a rdfs:Class,
        owl:Class ;
    dct:created "2024-12-17"^^xsd:date ;
    rdfs:isDefinedBy ieee-7012-owl: ;
    rdfs:subClassOf dpv-owl:ContractualClause ;
    sw:term_status "accepted"@en ;
    skos:definition "Term related to interpretation of the Term(s) using deontic logic"@en ;
    skos:prefLabel "Deontic Interpretation Term"@en .

ieee-7012-owl:Endpoint a rdfs:Class,
        owl:Class ;
    dct:created "2024-12-17"^^xsd:date ;
    dct:modified "2026-02-03"^^xsd:date ;
    rdfs:isDefinedBy ieee-7012-owl: ;
    rdfs:subClassOf dpv-owl:Location ;
    sw:term_status "modified"@en ;
    skos:definition "A location that acts as an endpoint, such as a URL, for carrying out communications and interactions between parties as defined in IEEE 7012"@en ;
    skos:prefLabel "Endpoint"@en .

ieee-7012-owl:Entity a rdfs:Class,
        owl:Class ;
    dct:created "2024-12-17"^^xsd:date ;
    rdfs:isDefinedBy ieee-7012-owl: ;
    rdfs:subClassOf dpv-owl:Organisation ;
    sw:term_status "accepted"@en ;
    skos:definition "An entity is any organisation with which a person makes or intends to make a contractual agreement, and which is the second party in a contract"@en ;
    skos:prefLabel "Entity"@en .

ieee-7012-owl:EntityAgent a rdfs:Class,
        owl:Class ;
    dct:created "2024-12-17"^^xsd:date ;
    rdfs:isDefinedBy ieee-7012-owl: ;
    rdfs:subClassOf ieee-7012-owl:Agent ;
    sw:term_status "accepted"@en ;
    skos:definition "An Agent that represents the Entity"@en ;
    skos:prefLabel "Entity Agent"@en .

ieee-7012-owl:NonServiceData a rdfs:Class,
        owl:Class,
        dpv-owl:PersonalData ;
    dct:created "2024-12-17"^^xsd:date ;
    rdfs:isDefinedBy ieee-7012-owl: ;
    rdfs:subClassOf dpv-owl:PersonalData ;
    sw:term_status "accepted"@en ;
    skos:definition "Data other than what is collected, produced, or otherwise generated in the context of a Service"@en ;
    skos:prefLabel "Non-Service Data"@en .

ieee-7012-owl:PDC a rdfs:Class,
        owl:Class,
        ieee-7012-owl:Agreement ;
    dct:created "2024-12-17"^^xsd:date ;
    rdfs:isDefinedBy ieee-7012-owl: ;
    rdfs:subClassOf ieee-7012-owl:Agreement ;
    sw:term_status "accepted"@en ;
    skos:definition "Term that indicates access is proactively provided by the person"@en ;
    skos:prefLabel "Personal Data Contribution"@en .

ieee-7012-owl:PDC-AI a rdfs:Class,
        owl:Class,
        ieee-7012-owl:Agreement ;
    dct:created "2024-12-17"^^xsd:date ;
    rdfs:isDefinedBy ieee-7012-owl: ;
    rdfs:subClassOf ieee-7012-owl:PDC ;
    sw:term_status "accepted"@en ;
    skos:definition "Term that indicates access to data is being provided for the purposes of Training and Operating AI technologies"@en ;
    skos:prefLabel "Personal Data Contribution for AI Training and Development"@en .

ieee-7012-owl:PDC-GOOD a rdfs:Class,
        owl:Class,
        ieee-7012-owl:Agreement ;
    dct:created "2024-12-17"^^xsd:date ;
    rdfs:isDefinedBy ieee-7012-owl: ;
    rdfs:subClassOf ieee-7012-owl:PDC ;
    sw:term_status "accepted"@en ;
    skos:definition "Term that indicates access to data is being provided for the purposes of Public Good"@en ;
    skos:prefLabel "Personal Data Contribution for Public Good"@en .

ieee-7012-owl:PDC-INTENT a rdfs:Class,
        owl:Class,
        ieee-7012-owl:Agreement ;
    dct:created "2024-12-17"^^xsd:date ;
    rdfs:isDefinedBy ieee-7012-owl: ;
    rdfs:subClassOf ieee-7012-owl:PDC ;
    sw:term_status "accepted"@en ;
    skos:definition "Term that indicates access to data is being provided for the purposes of Intent Casting"@en ;
    skos:prefLabel "Personal Data Contribution for Intent Casting"@en .

ieee-7012-owl:PartyTransparencyExAnte a rdfs:Class,
        owl:Class,
        dpv-owl:Obligation,
        ieee-7012-owl:PartyTransparencyTerm ;
    dct:created "2024-12-17"^^xsd:date ;
    rdfs:isDefinedBy ieee-7012-owl: ;
    rdfs:subClassOf ieee-7012-owl:PartyTransparencyRequired ;
    sw:term_status "accepted"@en ;
    skos:definition "Term that indicates transparency regarding identities and involvement of parties in specific roles is obligated ahead of intended process i.e. ex-ante transparency regarding identities and involvement of parties in specific roles"@en ;
    skos:prefLabel "Party Transparency Ex Ante"@en .

ieee-7012-owl:PartyTransparencyExPost a rdfs:Class,
        owl:Class,
        dpv-owl:Obligation,
        ieee-7012-owl:PartyTransparencyTerm ;
    dct:created "2024-12-17"^^xsd:date ;
    rdfs:isDefinedBy ieee-7012-owl: ;
    rdfs:subClassOf ieee-7012-owl:PartyTransparencyRequired ;
    sw:term_status "accepted"@en ;
    skos:definition "Term that indicates transparency regarding identities and involvement of parties in specific roles is obligated after intended process i.e. ex-post transparency regarding identities and involvement of parties in specific roles"@en ;
    skos:prefLabel "Party Transparency Ex Post"@en .

ieee-7012-owl:PartyTransparencyNotRequired a rdfs:Class,
        owl:Class,
        ieee-7012-owl:PartyTransparencyTerm ;
    dct:created "2024-12-17"^^xsd:date ;
    rdfs:isDefinedBy ieee-7012-owl: ;
    rdfs:subClassOf ieee-7012-owl:PartyTransparencyTerm ;
    sw:term_status "accepted"@en ;
    skos:definition "Term that indicates transparency regarding identities and involvement of parties in specific roles is not required to be provided"@en ;
    skos:prefLabel "Party Transparency Not Required"@en .

ieee-7012-owl:PartyTransparencyOnRequest a rdfs:Class,
        owl:Class,
        dpv-owl:Obligation,
        ieee-7012-owl:PartyTransparencyTerm ;
    dct:created "2024-12-17"^^xsd:date ;
    rdfs:isDefinedBy ieee-7012-owl: ;
    rdfs:subClassOf ieee-7012-owl:PartyTransparencyRequired ;
    sw:term_status "accepted"@en ;
    skos:definition "Term that indicates transparency regarding identities and involvement of parties in specific roles is obligated upon request"@en ;
    skos:prefLabel "Party Transparency On Request"@en .

ieee-7012-owl:PartyTransparencyRequired a rdfs:Class,
        owl:Class,
        dpv-owl:Obligation,
        ieee-7012-owl:PartyTransparencyTerm ;
    dct:created "2024-12-17"^^xsd:date ;
    rdfs:isDefinedBy ieee-7012-owl: ;
    rdfs:subClassOf dpv-owl:Obligation,
        ieee-7012-owl:PartyTransparencyTerm ;
    sw:term_status "accepted"@en ;
    skos:definition "Term that indicates transparency regarding identities and involvement of parties in specific roles is obligated"@en ;
    skos:prefLabel "Party Transparency Required"@en .

ieee-7012-owl:PartyTransparencyTerm a rdfs:Class,
        owl:Class ;
    dct:created "2024-12-17"^^xsd:date ;
    rdfs:isDefinedBy ieee-7012-owl: ;
    rdfs:subClassOf ieee-7012-owl:TransparencyTerm ;
    sw:term_status "accepted"@en ;
    skos:definition "Term that indicates transparency regarding identities and involvement of parties in specific roles as an obligation"@en ;
    skos:prefLabel "Party Transparency Term"@en .

ieee-7012-owl:PermissiveInterpretation a rdfs:Class,
        owl:Class,
        ieee-7012-owl:DeonticInterpretationTerm ;
    dct:created "2024-12-17"^^xsd:date ;
    rdfs:isDefinedBy ieee-7012-owl: ;
    rdfs:subClassOf ieee-7012-owl:DeonticInterpretationTerm ;
    sw:term_status "accepted"@en ;
    skos:definition "Term that indicates a permissive interpretation where if something is not prohibited or if there are no rules governing it, then it is assumed to be permitted"@en ;
    skos:prefLabel "Permissive Interpretation"@en .

ieee-7012-owl:Person a rdfs:Class,
        owl:Class ;
    dct:created "2024-12-17"^^xsd:date ;
    rdfs:isDefinedBy ieee-7012-owl: ;
    rdfs:subClassOf dpv-owl:NaturalPerson ;
    sw:term_status "accepted"@en ;
    skos:definition "The human individual or person whose personal data or privacy is involved, and which is the first party in a contract"@en ;
    skos:prefLabel "Person"@en .

ieee-7012-owl:PersonAgent a rdfs:Class,
        owl:Class ;
    dct:created "2024-12-17"^^xsd:date ;
    rdfs:isDefinedBy ieee-7012-owl: ;
    rdfs:subClassOf ieee-7012-owl:Agent ;
    sw:term_status "accepted"@en ;
    skos:definition "An Agent that represents the Person"@en ;
    skos:prefLabel "Person Agent"@en .

ieee-7012-owl:PortabilityNotRequired a rdfs:Class,
        owl:Class,
        dpv-owl:Obligation,
        ieee-7012-owl:PortabilityTerm ;
    dct:created "2024-12-17"^^xsd:date ;
    rdfs:isDefinedBy ieee-7012-owl: ;
    rdfs:subClassOf dpv-owl:Obligation,
        ieee-7012-owl:PortabilityTerm ;
    sw:term_status "accepted"@en ;
    skos:definition "Term that indicates data portability is not required to be provided"@en ;
    skos:prefLabel "Portability Not Required"@en .

ieee-7012-owl:PortabilityRequired a rdfs:Class,
        owl:Class,
        dpv-owl:Obligation,
        ieee-7012-owl:PortabilityTerm ;
    dct:created "2024-12-17"^^xsd:date ;
    rdfs:isDefinedBy ieee-7012-owl: ;
    rdfs:subClassOf dpv-owl:Obligation,
        ieee-7012-owl:PortabilityTerm ;
    sw:term_status "accepted"@en ;
    skos:definition "Term that indicates data portability is required to be provided"@en ;
    skos:prefLabel "Portability Required"@en .

ieee-7012-owl:PortabilityRequiredImmediately a rdfs:Class,
        owl:Class,
        dpv-owl:Obligation,
        ieee-7012-owl:PortabilityTerm ;
    dct:created "2024-12-17"^^xsd:date ;
    rdfs:isDefinedBy ieee-7012-owl: ;
    rdfs:subClassOf ieee-7012-owl:PortabilityRequired ;
    sw:term_status "accepted"@en ;
    skos:definition "Term that indicates data should be ported or made available immediately without delay"@en ;
    skos:prefLabel "Portability Required Immediately"@en .

ieee-7012-owl:PortabilityRequiredOnRequest a rdfs:Class,
        owl:Class,
        dpv-owl:Obligation,
        ieee-7012-owl:PortabilityTerm ;
    dct:created "2024-12-17"^^xsd:date ;
    rdfs:isDefinedBy ieee-7012-owl: ;
    rdfs:subClassOf ieee-7012-owl:PortabilityRequired ;
    sw:term_status "accepted"@en ;
    skos:definition "Term that indicates data should be ported or made available on request"@en ;
    skos:prefLabel "Portability Required On Request"@en .

ieee-7012-owl:PortabilityTerm a rdfs:Class,
        owl:Class ;
    dct:created "2024-12-17"^^xsd:date ;
    rdfs:isDefinedBy ieee-7012-owl: ;
    rdfs:subClassOf dpv-owl:ContractualClause ;
    sw:term_status "accepted"@en ;
    skos:definition "Term that indicates portability of data from service provider to individual"@en ;
    skos:prefLabel "Portability Term"@en ;
    ieee-7012-owl:hasHumanDescription "Data portability means that you are entitled to ask organisations that hold records about you (your personal data) to be sent in a modern, useful format either to you directly, or to another organisation/ app that you nominate. Examples of that might be your bank transactions (via Open Banking or similar), your home energy use, your vehicle use and many more." .

ieee-7012-owl:PortabilityToThirdParty a rdfs:Class,
        owl:Class,
        dpv-owl:Obligation,
        ieee-7012-owl:PortabilityTerm ;
    dct:created "2024-12-17"^^xsd:date ;
    rdfs:isDefinedBy ieee-7012-owl: ;
    rdfs:subClassOf ieee-7012-owl:PortabilityRequired ;
    sw:term_status "accepted"@en ;
    skos:definition "Term that indicates data should be ported or made available to third party"@en ;
    skos:prefLabel "Portability To Third Party"@en .

ieee-7012-owl:PreferenceAlwaysApplies a rdfs:Class,
        owl:Class,
        ieee-7012-owl:PreferenceApplicability ;
    dct:created "2024-12-17"^^xsd:date ;
    rdfs:isDefinedBy ieee-7012-owl: ;
    rdfs:subClassOf ieee-7012-owl:PreferenceApplicability ;
    sw:term_status "accepted"@en ;
    skos:definition "Term that indicates the privacy preference always applies in all contexts and should always be used in agreements and negotiations"@en ;
    skos:prefLabel "Preference Always Applies"@en .

ieee-7012-owl:PreferenceApplicability a rdfs:Class,
        owl:Class ;
    dct:created "2024-12-17"^^xsd:date ;
    rdfs:isDefinedBy ieee-7012-owl: ;
    rdfs:subClassOf dpv-owl:ContractualClause ;
    sw:term_status "accepted"@en ;
    skos:definition "Term that indicates the applicability of Privacy Preference(s)"@en ;
    skos:prefLabel "Privacy Preference Applicability"@en .

ieee-7012-owl:PreferenceConditionallyApplies a rdfs:Class,
        owl:Class,
        ieee-7012-owl:PreferenceApplicability ;
    dct:created "2024-12-17"^^xsd:date ;
    rdfs:isDefinedBy ieee-7012-owl: ;
    rdfs:subClassOf ieee-7012-owl:PreferenceApplicability ;
    sw:term_status "accepted"@en ;
    skos:definition "Term that indicates the privacy preference conditionally applies i.e. it should only be used in agreements and negotiations if the associated condition is satisfied within the context"@en ;
    skos:prefLabel "Preference Conditionally Applies"@en .

ieee-7012-owl:PreferenceNeverApplies a rdfs:Class,
        owl:Class,
        ieee-7012-owl:PreferenceApplicability ;
    dct:created "2024-12-17"^^xsd:date ;
    rdfs:isDefinedBy ieee-7012-owl: ;
    rdfs:subClassOf ieee-7012-owl:PreferenceApplicability ;
    sw:term_status "accepted"@en ;
    skos:definition "Term that indicates the privacy preference never applies in any context and should never be used in agreements or negotiations"@en ;
    skos:prefLabel "Preference Never Applies"@en .

ieee-7012-owl:Profiling2PAllowed a rdfs:Class,
        owl:Class,
        dpv-owl:Permission,
        ieee-7012-owl:ProfilingTerm ;
    dct:created "2024-12-17"^^xsd:date ;
    rdfs:isDefinedBy ieee-7012-owl: ;
    rdfs:subClassOf ieee-7012-owl:ProfilingAllowed ;
    sw:term_status "accepted"@en ;
    skos:definition "Term that indicates Profiling is allowed but only by the 1st Party"@en ;
    skos:prefLabel "Profiling Allowed Only First Party"@en .

ieee-7012-owl:Profiling3PDisallowed a rdfs:Class,
        owl:Class,
        dpv-owl:Prohibition,
        ieee-7012-owl:ProfilingTerm ;
    dct:created "2024-12-17"^^xsd:date ;
    rdfs:isDefinedBy ieee-7012-owl: ;
    rdfs:subClassOf ieee-7012-owl:ProfilingDisallowed ;
    sw:term_status "accepted"@en ;
    skos:definition "Term that indicates Profiling is not allowed by 3rd Parties"@en ;
    skos:prefLabel "Profiling Disallowed For Third Party"@en .

ieee-7012-owl:ProfilingAllowed a rdfs:Class,
        owl:Class,
        dpv-owl:Permission,
        ieee-7012-owl:ProfilingTerm ;
    dct:created "2024-12-17"^^xsd:date ;
    rdfs:isDefinedBy ieee-7012-owl: ;
    rdfs:subClassOf dpv-owl:Permission,
        ieee-7012-owl:ProfilingTerm ;
    sw:term_status "accepted"@en ;
    skos:definition "Term that indicates Profiling is allowed"@en ;
    skos:prefLabel "Profiling Allowed"@en .

ieee-7012-owl:ProfilingDisallowed a rdfs:Class,
        owl:Class,
        dpv-owl:Prohibition,
        ieee-7012-owl:ProfilingTerm ;
    dct:created "2024-12-17"^^xsd:date ;
    rdfs:isDefinedBy ieee-7012-owl: ;
    rdfs:subClassOf dpv-owl:Prohibition,
        ieee-7012-owl:ProfilingTerm ;
    sw:term_status "accepted"@en ;
    skos:definition "Term that indicates Profiling is not allowed"@en ;
    skos:prefLabel "Profiling Disallowed"@en .

ieee-7012-owl:ProfilingTerm a rdfs:Class,
        owl:Class ;
    dct:created "2024-12-17"^^xsd:date ;
    rdfs:isDefinedBy ieee-7012-owl: ;
    rdfs:subClassOf dpv-owl:ContractualClause ;
    sw:term_status "accepted"@en ;
    skos:definition "Term related to Profiling"@en ;
    skos:prefLabel "Profiling Term"@en .

ieee-7012-owl:ProfilingWithFPDisallowed a rdfs:Class,
        owl:Class,
        dpv-owl:Prohibition,
        ieee-7012-owl:ProfilingTerm ;
    dct:created "2024-12-17"^^xsd:date ;
    rdfs:isDefinedBy ieee-7012-owl: ;
    rdfs:subClassOf ieee-7012-owl:ProfilingDisallowed ;
    sw:term_status "accepted"@en ;
    skos:definition "Term that indicates Profiling involving use of Fingerprinting is not allowed"@en ;
    skos:prefLabel "Profiling Disallowed FP"@en .

ieee-7012-owl:ProfilingWithPIIDisallowed a rdfs:Class,
        owl:Class,
        dpv-owl:Prohibition,
        ieee-7012-owl:ProfilingTerm ;
    dct:created "2024-12-17"^^xsd:date ;
    rdfs:isDefinedBy ieee-7012-owl: ;
    rdfs:subClassOf ieee-7012-owl:ProfilingDisallowed ;
    sw:term_status "accepted"@en ;
    skos:definition "Term that indicates Profiling involving use of PII is not allowed"@en ;
    skos:prefLabel "Profiling Disallowed PII"@en .

ieee-7012-owl:ProfilingWithoutFPAllowed a rdfs:Class,
        owl:Class,
        dpv-owl:Permission,
        ieee-7012-owl:ProfilingTerm ;
    dct:created "2024-12-17"^^xsd:date ;
    rdfs:isDefinedBy ieee-7012-owl: ;
    rdfs:subClassOf ieee-7012-owl:ProfilingAllowed ;
    sw:term_status "accepted"@en ;
    skos:definition "Term that indicates Profiling is allowed but only if it does not involve Fingerprinting"@en ;
    skos:prefLabel "Profiling Allowed No FP"@en .

ieee-7012-owl:ProfilingWithoutPIIAllowed a rdfs:Class,
        owl:Class,
        dpv-owl:Permission,
        ieee-7012-owl:ProfilingTerm ;
    dct:created "2024-12-17"^^xsd:date ;
    rdfs:isDefinedBy ieee-7012-owl: ;
    rdfs:subClassOf ieee-7012-owl:ProfilingAllowed ;
    sw:term_status "accepted"@en ;
    skos:definition "Term that indicates Profiling is allowed but only if it uses non-PII"@en ;
    skos:prefLabel "Profiling Allowed Only Non PII"@en .

ieee-7012-owl:ProhibitiveInterpretation a rdfs:Class,
        owl:Class,
        ieee-7012-owl:DeonticInterpretationTerm ;
    dct:created "2024-12-17"^^xsd:date ;
    rdfs:isDefinedBy ieee-7012-owl: ;
    rdfs:subClassOf ieee-7012-owl:DeonticInterpretationTerm ;
    sw:term_status "accepted"@en ;
    skos:definition "Term that indicates a prohibitive interpretation where if something is not permitted or if there are no rules governing it, then it is assumed to be prohibited"@en ;
    skos:prefLabel "Prohibitive Interpretation"@en .

ieee-7012-owl:PurposeTransparencyExAnte a rdfs:Class,
        owl:Class,
        dpv-owl:Obligation,
        ieee-7012-owl:PurposeTransparencyTerm ;
    dct:created "2024-12-17"^^xsd:date ;
    rdfs:isDefinedBy ieee-7012-owl: ;
    rdfs:subClassOf ieee-7012-owl:PurposeTransparencyRequired ;
    sw:term_status "accepted"@en ;
    skos:definition "Term that indicates transparency regarding purposes involved for processing of data and technologies is obligated ahead of intended process i.e. ex-ante transparency regarding purposes involved for processing of data and technologies"@en ;
    skos:prefLabel "Purpose Transparency Ex Ante"@en .

ieee-7012-owl:PurposeTransparencyExPost a rdfs:Class,
        owl:Class,
        dpv-owl:Obligation,
        ieee-7012-owl:PurposeTransparencyTerm ;
    dct:created "2024-12-17"^^xsd:date ;
    rdfs:isDefinedBy ieee-7012-owl: ;
    rdfs:subClassOf ieee-7012-owl:PurposeTransparencyRequired ;
    sw:term_status "accepted"@en ;
    skos:definition "Term that indicates transparency regarding purposes involved for processing of data and technologies is obligated after intended process i.e. ex-post transparency regarding purposes involved for processing of data and technologies"@en ;
    skos:prefLabel "Purpose Transparency Ex Post"@en .

ieee-7012-owl:PurposeTransparencyNotRequired a rdfs:Class,
        owl:Class,
        ieee-7012-owl:PurposeTransparencyTerm ;
    dct:created "2024-12-17"^^xsd:date ;
    rdfs:isDefinedBy ieee-7012-owl: ;
    rdfs:subClassOf ieee-7012-owl:PurposeTransparencyTerm ;
    sw:term_status "accepted"@en ;
    skos:definition "Term that indicates transparency regarding purposes involved for processing of data and technologies is not required to be provided"@en ;
    skos:prefLabel "Purpose Transparency Not Required"@en .

ieee-7012-owl:PurposeTransparencyOnRequest a rdfs:Class,
        owl:Class,
        dpv-owl:Obligation,
        ieee-7012-owl:PurposeTransparencyTerm ;
    dct:created "2024-12-17"^^xsd:date ;
    rdfs:isDefinedBy ieee-7012-owl: ;
    rdfs:subClassOf ieee-7012-owl:PurposeTransparencyRequired ;
    sw:term_status "accepted"@en ;
    skos:definition "Term that indicates transparency regarding purposes involved for processing of data and technologies is obligated upon request"@en ;
    skos:prefLabel "Purpose Transparency On Request"@en .

ieee-7012-owl:PurposeTransparencyRequired a rdfs:Class,
        owl:Class,
        dpv-owl:Obligation,
        ieee-7012-owl:PurposeTransparencyTerm ;
    dct:created "2024-12-17"^^xsd:date ;
    rdfs:isDefinedBy ieee-7012-owl: ;
    rdfs:subClassOf dpv-owl:Obligation,
        ieee-7012-owl:PurposeTransparencyTerm ;
    sw:term_status "accepted"@en ;
    skos:definition "Term that indicates transparency regarding purposes is obligated"@en ;
    skos:prefLabel "Purpose Transparency Required"@en .

ieee-7012-owl:PurposeTransparencyTerm a rdfs:Class,
        owl:Class ;
    dct:created "2024-12-17"^^xsd:date ;
    rdfs:isDefinedBy ieee-7012-owl: ;
    rdfs:subClassOf ieee-7012-owl:TransparencyTerm ;
    sw:term_status "accepted"@en ;
    skos:definition "Term that indicates transparency regarding purposes involved for processing of data and technologies as an obligation"@en ;
    skos:prefLabel "Purpose Transparency Term"@en .

ieee-7012-owl:ResolveAcrossContexts a rdfs:Class,
        owl:Class,
        ieee-7012-owl:ConflictResolutionTerm ;
    dct:created "2024-12-17"^^xsd:date ;
    rdfs:isDefinedBy ieee-7012-owl: ;
    rdfs:subClassOf ieee-7012-owl:ConflictResolutionTerm ;
    sw:term_status "accepted"@en ;
    skos:definition "Term that indicates this conflict method should be used to resolve all conflicts across contexts i.e. other contexts that have their own conflict resolution method should be overridden"@en ;
    skos:prefLabel "Resolve Across Contexts"@en .

ieee-7012-owl:ResolveByDiscarding a rdfs:Class,
        owl:Class,
        ieee-7012-owl:ConflictResolutionTerm ;
    dct:created "2024-12-17"^^xsd:date ;
    rdfs:isDefinedBy ieee-7012-owl: ;
    rdfs:subClassOf ieee-7012-owl:ConflictResolutionTerm ;
    sw:term_status "accepted"@en ;
    skos:definition "Term that indicates a conflict should be resolved by discarding the conflicting terms i.e. removing all terms that are in conflict"@en ;
    skos:prefLabel "Resolve By Discarding"@en .

ieee-7012-owl:ResolveOnlyWithinContext a rdfs:Class,
        owl:Class,
        ieee-7012-owl:ConflictResolutionTerm ;
    dct:created "2024-12-17"^^xsd:date ;
    rdfs:isDefinedBy ieee-7012-owl: ;
    rdfs:subClassOf ieee-7012-owl:ConflictResolutionTerm ;
    sw:term_status "accepted"@en ;
    skos:definition "Term that indicates a conflict should be resolved using the specified method but only for this context i.e. other contexts that have their own conflict resolution method should not be overridden"@en ;
    skos:prefLabel "Resolve Only Within Context"@en .

ieee-7012-owl:ResolvePreferringPermission a rdfs:Class,
        owl:Class,
        ieee-7012-owl:ConflictResolutionTerm ;
    dct:created "2024-12-17"^^xsd:date ;
    rdfs:isDefinedBy ieee-7012-owl: ;
    rdfs:subClassOf ieee-7012-owl:ConflictResolutionTerm ;
    sw:term_status "accepted"@en ;
    skos:definition "Term that indicates a conflict should be resolved by preferring the permission over the prohibition i.e. if something is both prohibited and permitted, it is assumed to be permitted"@en ;
    skos:prefLabel "Resolve Preferring Permission"@en .

ieee-7012-owl:ResolvePreferringProhibition a rdfs:Class,
        owl:Class,
        ieee-7012-owl:ConflictResolutionTerm ;
    dct:created "2024-12-17"^^xsd:date ;
    rdfs:isDefinedBy ieee-7012-owl: ;
    rdfs:subClassOf ieee-7012-owl:ConflictResolutionTerm ;
    sw:term_status "accepted"@en ;
    skos:definition "Term that indicates a conflict should be resolved by preferring the prohibition over the permission i.e. if something is both prohibited and permitted, it is assumed to be prohibited"@en ;
    skos:prefLabel "Resolve Preferring Prohibition"@en .

ieee-7012-owl:SD-BASE a rdfs:Class,
        owl:Class,
        ieee-7012-owl:Agreement ;
    dct:created "2024-12-17"^^xsd:date ;
    rdfs:isDefinedBy ieee-7012-owl: ;
    rdfs:subClassOf ieee-7012-owl:Agreement ;
    sw:term_status "accepted"@en ;
    skos:definition "Term that requires Service Delivery, and prohibits Analytics, Tracking, or Profiling by 2nd and 3rd Party, and prohibits sharing any data with 3rd Party"@en ;
    skos:prefLabel "SD-BASE"@en ;
    dpv-owl:hasObligation ieee-7012-owl:ServiceDeliveryRequired ;
    dpv-owl:hasProhibition ieee-7012-owl:AnalyticsDisallowed,
        ieee-7012-owl:DataSharingDisallowed,
        ieee-7012-owl:ProfilingDisallowed,
        ieee-7012-owl:TrackingDisallowed .

ieee-7012-owl:SD-BASE-A a rdfs:Class,
        owl:Class,
        ieee-7012-owl:Agreement ;
    dct:created "2024-12-17"^^xsd:date ;
    rdfs:isDefinedBy ieee-7012-owl: ;
    rdfs:subClassOf ieee-7012-owl:SD-BASE ;
    sw:term_status "accepted"@en ;
    skos:definition "Term that requires Service Delivery and permits Analytics, and prohibits Analytics by 3rd Party, prohibits Tracking, or Profiling by 2nd and 3rd Party, and prohibits sharing any data with 3rd Party"@en ;
    skos:prefLabel "SD BASE-A"@en ;
    dpv-owl:hasObligation ieee-7012-owl:ServiceDeliveryRequired ;
    dpv-owl:hasPermission ieee-7012-owl:Analytics2PAllowed ;
    dpv-owl:hasProhibition ieee-7012-owl:Analytics3PDisallowed,
        ieee-7012-owl:DataSharingDisallowed,
        ieee-7012-owl:ProfilingDisallowed,
        ieee-7012-owl:TrackingDisallowed .

ieee-7012-owl:SD-BASE-A-DP a rdfs:Class,
        owl:Class,
        ieee-7012-owl:Agreement ;
    dct:created "2024-12-17"^^xsd:date ;
    rdfs:isDefinedBy ieee-7012-owl: ;
    rdfs:subClassOf ieee-7012-owl:SD-BASE-A,
        ieee-7012-owl:SD-BASE-DP ;
    sw:term_status "accepted"@en ;
    skos:definition "Term that requires Service Delivery and permits Analytics, with an obligation for Data Portability, and prohibits Analytics by 3rd Party, prohibits Tracking or Profiling by 2nd and 3rd Party, and prohibits sharing any data with 3rd Party"@en ;
    skos:prefLabel "SD BASE-A-DP"@en ;
    dpv-owl:hasObligation ieee-7012-owl:PortabilityRequired,
        ieee-7012-owl:ServiceDeliveryRequired ;
    dpv-owl:hasPermission ieee-7012-owl:Analytics2PAllowed ;
    dpv-owl:hasProhibition ieee-7012-owl:Analytics3PDisallowed,
        ieee-7012-owl:DataSharingDisallowed,
        ieee-7012-owl:ProfilingDisallowed,
        ieee-7012-owl:TrackingDisallowed .

ieee-7012-owl:SD-BASE-AT a rdfs:Class,
        owl:Class,
        ieee-7012-owl:Agreement ;
    dct:created "2024-12-17"^^xsd:date ;
    rdfs:isDefinedBy ieee-7012-owl: ;
    rdfs:subClassOf ieee-7012-owl:SD-BASE-A ;
    sw:term_status "accepted"@en ;
    skos:definition "Term that requires Service Delivery, and permits Analytics and Tracking by the 2nd Party, and prohibits Analytics, or Tracking by 3rd Party, prohibits Profiling by 2nd and 3rd Party, and prohibits sharing any data with 3rd Party"@en ;
    skos:prefLabel "SD BASE-AT"@en ;
    dpv-owl:hasObligation ieee-7012-owl:ServiceDeliveryRequired ;
    dpv-owl:hasPermission ieee-7012-owl:Analytics2PAllowed,
        ieee-7012-owl:Tracking2PAllowed ;
    dpv-owl:hasProhibition ieee-7012-owl:Analytics3PDisallowed,
        ieee-7012-owl:DataSharingDisallowed,
        ieee-7012-owl:ProfilingDisallowed,
        ieee-7012-owl:Tracking3PDisallowed .

ieee-7012-owl:SD-BASE-AT-DP a rdfs:Class,
        owl:Class,
        ieee-7012-owl:Agreement ;
    dct:created "2024-12-17"^^xsd:date ;
    rdfs:isDefinedBy ieee-7012-owl: ;
    rdfs:subClassOf ieee-7012-owl:SD-BASE-AT,
        ieee-7012-owl:SD-BASE-DP ;
    sw:term_status "accepted"@en ;
    skos:definition "Term that requires Service Delivery, and permits Analytics and Tracking by the 2nd Party, with an obligation for Data Portability, and prohibits Analytics or Tracking by 3rd Party, prohibits Profiling by 2nd and 3rd Party, and prohibits sharing any data with 3rd Party"@en ;
    skos:prefLabel "SD BASE-AT-DP"@en ;
    dpv-owl:hasObligation ieee-7012-owl:PortabilityRequired,
        ieee-7012-owl:ServiceDeliveryRequired ;
    dpv-owl:hasPermission ieee-7012-owl:Analytics2PAllowed,
        ieee-7012-owl:Tracking2PAllowed ;
    dpv-owl:hasProhibition ieee-7012-owl:Analytics3PDisallowed,
        ieee-7012-owl:DataSharingDisallowed,
        ieee-7012-owl:ProfilingDisallowed,
        ieee-7012-owl:Tracking3PDisallowed .

ieee-7012-owl:SD-BASE-ATP a rdfs:Class,
        owl:Class,
        ieee-7012-owl:Agreement ;
    dct:created "2024-12-17"^^xsd:date ;
    rdfs:isDefinedBy ieee-7012-owl: ;
    rdfs:subClassOf ieee-7012-owl:SD-BASE-AT ;
    sw:term_status "accepted"@en ;
    skos:definition "Term that requires Service Delivery, and permits Analytics, Tracking, or Profiling by the 2nd party, and prohibits Analytics, Tracking, or Profiling by 3rd Party, and prohibits sharing any data with 3rd Party"@en ;
    skos:prefLabel "SD BASE-ATP"@en ;
    dpv-owl:hasObligation ieee-7012-owl:ServiceDeliveryRequired ;
    dpv-owl:hasPermission ieee-7012-owl:Analytics2PAllowed,
        ieee-7012-owl:Profiling2PAllowed,
        <https://w3id.org/dpv/standards/ieee/7012/owl#Tracking2PAllowed
> ;
    dpv-owl:hasProhibition ieee-7012-owl:Analytics3PDisallowed,
        ieee-7012-owl:DataSharingDisallowed,
        ieee-7012-owl:Profiling3PDisallowed,
        ieee-7012-owl:Tracking3PDisallowed .

ieee-7012-owl:SD-BASE-ATP-DP a rdfs:Class,
        owl:Class,
        ieee-7012-owl:Agreement ;
    dct:created "2024-12-17"^^xsd:date ;
    rdfs:isDefinedBy ieee-7012-owl: ;
    rdfs:subClassOf ieee-7012-owl:SD-BASE-ATP,
        ieee-7012-owl:SD-BASE-DP ;
    sw:term_status "accepted"@en ;
    skos:definition "Term that requires Service Delivery, and permits Analytics, Tracking, or Profiling by the 2nd Party, with an obligation for Data Portability, and prohibits Analytics, Tracking, or Profiling by 3rd Party, and prohibits sharing any data with 3rd Party"@en ;
    skos:prefLabel "SD BASE-ATP-DP"@en ;
    dpv-owl:hasObligation ieee-7012-owl:PortabilityRequired,
        ieee-7012-owl:ServiceDeliveryRequired ;
    dpv-owl:hasPermission ieee-7012-owl:Analytics2PAllowed,
        ieee-7012-owl:Profiling2PAllowed,
        <https://w3id.org/dpv/standards/ieee/7012/owl#Tracking2PAllowed
> ;
    dpv-owl:hasProhibition ieee-7012-owl:Analytics3PDisallowed,
        ieee-7012-owl:DataSharingDisallowed,
        ieee-7012-owl:Profiling3PDisallowed,
        ieee-7012-owl:Tracking3PDisallowed .

ieee-7012-owl:SD-BASE-ATP-S3P a rdfs:Class,
        owl:Class,
        ieee-7012-owl:Agreement ;
    dct:created "2024-12-17"^^xsd:date ;
    rdfs:isDefinedBy ieee-7012-owl: ;
    rdfs:subClassOf ieee-7012-owl:SD-BASE-ATP ;
    sw:term_status "accepted"@en ;
    skos:definition "Term that requires Service Delivery, and permits Analytics, Tracking, or Profiling by the 2nd Party, and permits sharing data that has been fully anonymised with 3rd Party, and prohibits Analytics, Tracking, or Profiling by 3rd Party, and prohibits sharing on non-anonymised data with 3rd Party"@en ;
    skos:prefLabel "SD BASE-ATP-S3P"@en ;
    dpv-owl:hasObligation ieee-7012-owl:ServiceDeliveryRequired ;
    dpv-owl:hasPermission ieee-7012-owl:Analytics2PAllowed,
        ieee-7012-owl:DataSharingAnonymised3PAllowed,
        ieee-7012-owl:Profiling2PAllowed,
        <https://w3id.org/dpv/standards/ieee/7012/owl#Tracking2PAllowed
> ;
    dpv-owl:hasProhibition ieee-7012-owl:Analytics3PDisallowed,
        ieee-7012-owl:Profiling3PDisallowed,
        ieee-7012-owl:SharingDataNonAnonymised3PDisallowed,
        ieee-7012-owl:Tracking3PDisallowed .

ieee-7012-owl:SD-BASE-ATP-S3P-DP a rdfs:Class,
        owl:Class,
        ieee-7012-owl:Agreement ;
    dct:created "2024-12-17"^^xsd:date ;
    rdfs:isDefinedBy ieee-7012-owl: ;
    rdfs:subClassOf ieee-7012-owl:SD-BASE-ATP-S3P,
        ieee-7012-owl:SD-BASE-DP ;
    sw:term_status "accepted"@en ;
    skos:definition "Term that requires Service Delivery, and permits Analytics, Tracking, or Profiling by the 2nd Party, and permits sharing data that has been fully anonymised with 3rd Party, with an obligation for Data Portability, and prohibits Analytics, Tracking, Profiling by 3rd Party, and prohibits sharing on non-anonymised data with 3rd Party"@en ;
    skos:prefLabel "SD BASE-ATP-S3P-DP"@en ;
    dpv-owl:hasObligation ieee-7012-owl:PortabilityRequired,
        ieee-7012-owl:ServiceDeliveryRequired ;
    dpv-owl:hasPermission ieee-7012-owl:Analytics2PAllowed,
        ieee-7012-owl:DataSharingAnonymised3PAllowed,
        ieee-7012-owl:Profiling2PAllowed,
        <https://w3id.org/dpv/standards/ieee/7012/owl#Tracking2PAllowed
> ;
    dpv-owl:hasProhibition ieee-7012-owl:Analytics3PDisallowed,
        ieee-7012-owl:Profiling3PDisallowed,
        ieee-7012-owl:SharingDataNonAnonymised3PDisallowed,
        ieee-7012-owl:Tracking3PDisallowed .

ieee-7012-owl:SD-BASE-DP a rdfs:Class,
        owl:Class,
        ieee-7012-owl:Agreement ;
    dct:created "2024-12-17"^^xsd:date ;
    rdfs:isDefinedBy ieee-7012-owl: ;
    rdfs:subClassOf ieee-7012-owl:SD-BASE ;
    sw:term_status "accepted"@en ;
    skos:definition "Term that requires Service Delivery, with an obligation for Data Portability, and prohibits Analytics, Tracking, or Profiling by 2nd and 3rd Party, and prohibits sharing any data with 3rd Party"@en ;
    skos:prefLabel "SD BASE-DP"@en ;
    dpv-owl:hasObligation ieee-7012-owl:PortabilityRequired,
        ieee-7012-owl:ServiceDeliveryRequired ;
    dpv-owl:hasProhibition ieee-7012-owl:AnalyticsDisallowed,
        ieee-7012-owl:DataSharingDisallowed,
        ieee-7012-owl:ProfilingDisallowed,
        ieee-7012-owl:TrackingDisallowed .

ieee-7012-owl:ServiceAnalytics a rdfs:Class,
        owl:Class,
        dpv-owl:Purpose ;
    dct:created "2024-12-17"^^xsd:date ;
    rdfs:isDefinedBy ieee-7012-owl: ;
    rdfs:subClassOf dpv-owl:ServiceUsageAnalytics ;
    sw:term_status "accepted"@en ;
    skos:definition "Purposes associated with analysing the usage, delivery, and provisioning metrics of a service"@en ;
    skos:prefLabel "Service Analytics"@en .

ieee-7012-owl:ServiceAnalyticsData a rdfs:Class,
        owl:Class,
        dpv-owl:PersonalData ;
    dct:created "2024-12-17"^^xsd:date ;
    rdfs:isDefinedBy ieee-7012-owl: ;
    rdfs:subClassOf dpv-owl:PersonalData ;
    sw:term_status "accepted"@en ;
    skos:definition "Data collected, produced, or otherwise generated in the context of analysing the usage and provision of a Service"@en ;
    skos:prefLabel "Service Analytics Data"@en .

ieee-7012-owl:ServiceData a rdfs:Class,
        owl:Class,
        dpv-owl:PersonalData ;
    dct:created "2024-12-17"^^xsd:date ;
    rdfs:isDefinedBy ieee-7012-owl: ;
    rdfs:subClassOf dpv-owl:PersonalData ;
    sw:term_status "accepted"@en ;
    skos:definition "Data collected, produced, or otherwise generated in the context of a Service"@en ;
    skos:prefLabel "Service Data"@en .

ieee-7012-owl:ServiceDelivery a rdfs:Class,
        owl:Class,
        dpv-owl:Purpose ;
    dct:created "2024-12-17"^^xsd:date ;
    rdfs:isDefinedBy ieee-7012-owl: ;
    rdfs:subClassOf dpv-owl:RequestedServiceProvision ;
    sw:term_status "accepted"@en ;
    skos:definition "Purposes associated with delivery of a service"@en ;
    skos:prefLabel "Service Delivery"@en .

ieee-7012-owl:ServiceImprovement a rdfs:Class,
        owl:Class,
        dpv-owl:Purpose ;
    dct:created "2024-12-17"^^xsd:date ;
    rdfs:isDefinedBy ieee-7012-owl: ;
    rdfs:subClassOf dpv-owl:ServiceOptimisation ;
    sw:term_status "accepted"@en ;
    skos:definition "Purposes associated with identifying and implementing improvements to a service"@en ;
    skos:prefLabel "Service Improvement"@en .

ieee-7012-owl:ServiceUsageData a rdfs:Class,
        owl:Class,
        dpv-owl:PersonalData ;
    dct:created "2024-12-17"^^xsd:date ;
    rdfs:isDefinedBy ieee-7012-owl: ;
    rdfs:subClassOf dpv-owl:PersonalData ;
    sw:term_status "accepted"@en ;
    skos:definition "Data collected, produced, or otherwise generated in the context of using a Service"@en ;
    skos:prefLabel "Service Usage Data"@en .

ieee-7012-owl:SharingData3PAllowed a rdfs:Class,
        owl:Class,
        dpv-owl:Permission,
        ieee-7012-owl:DataSharingTerm ;
    dct:created "2024-12-17"^^xsd:date ;
    rdfs:isDefinedBy ieee-7012-owl: ;
    rdfs:subClassOf ieee-7012-owl:SharingDataAllowed ;
    sw:term_status "accepted"@en ;
    skos:definition "Term that indicates data sharing with third party is allowed"@en ;
    skos:prefLabel "Sharing Data with 3rd Party Allowed"@en .

ieee-7012-owl:SharingData3PDisallowed a rdfs:Class,
        owl:Class,
        dpv-owl:Prohibition,
        ieee-7012-owl:DataSharingTerm ;
    dct:created "2024-12-17"^^xsd:date ;
    rdfs:isDefinedBy ieee-7012-owl: ;
    rdfs:subClassOf ieee-7012-owl:SharingDataDisallowed ;
    sw:term_status "accepted"@en ;
    skos:definition "Term that indicates data sharing with third party is disallowed"@en ;
    skos:prefLabel "Sharing Data with 3rd Party Disallowed"@en .

ieee-7012-owl:SharingDataAllowed a rdfs:Class,
        owl:Class,
        dpv-owl:Permission,
        ieee-7012-owl:DataSharingTerm ;
    dct:created "2024-12-17"^^xsd:date ;
    rdfs:isDefinedBy ieee-7012-owl: ;
    rdfs:subClassOf dpv-owl:Permission,
        ieee-7012-owl:DataSharingTerm ;
    sw:term_status "accepted"@en ;
    skos:definition "Term that indicates Data Sharing is allowed"@en ;
    skos:prefLabel "Sharing Data Allowed"@en .

ieee-7012-owl:SharingDataAnonymised3PAllowed a rdfs:Class,
        owl:Class,
        dpv-owl:Permission,
        ieee-7012-owl:DataSharingTerm ;
    dct:created "2024-12-17"^^xsd:date ;
    rdfs:isDefinedBy ieee-7012-owl: ;
    rdfs:subClassOf ieee-7012-owl:SharingDataAllowed ;
    sw:term_status "accepted"@en ;
    skos:definition "Term that indicates data sharing only of anonymised data with third party is allowed"@en ;
    skos:prefLabel "Sharing Anonymised Data with 3rd Party Allowed"@en .

ieee-7012-owl:SharingDataAnonymised3PDisallowed a rdfs:Class,
        owl:Class,
        dpv-owl:Prohibition,
        ieee-7012-owl:DataSharingTerm ;
    dct:created "2024-12-17"^^xsd:date ;
    rdfs:isDefinedBy ieee-7012-owl: ;
    rdfs:subClassOf ieee-7012-owl:SharingDataDisallowed ;
    sw:term_status "accepted"@en ;
    skos:definition "Term that indicates data sharing of full anonymised data with third party is disallowed"@en ;
    skos:prefLabel "Sharing Anonymised Data with 3rd Party Disallowed"@en .

ieee-7012-owl:SharingDataDisallowed a rdfs:Class,
        owl:Class,
        dpv-owl:Prohibition,
        ieee-7012-owl:DataSharingTerm ;
    dct:created "2024-12-17"^^xsd:date ;
    rdfs:isDefinedBy ieee-7012-owl: ;
    rdfs:subClassOf dpv-owl:Prohibition,
        ieee-7012-owl:DataSharingTerm ;
    sw:term_status "accepted"@en ;
    skos:definition "Term that indicates Data Sharing is not allowed"@en ;
    skos:prefLabel "Sharing Data Disallowed"@en .

ieee-7012-owl:SharingDataNonAnonymised3PDisallowed a rdfs:Class,
        owl:Class,
        dpv-owl:Prohibition,
        ieee-7012-owl:DataSharingTerm ;
    dct:created "2024-12-17"^^xsd:date ;
    rdfs:isDefinedBy ieee-7012-owl: ;
    rdfs:subClassOf ieee-7012-owl:SharingDataDisallowed ;
    sw:term_status "accepted"@en ;
    skos:definition "Term that indicates data sharing of non-anonymised data with third party is disallowed"@en ;
    skos:prefLabel "Sharing Non-Anonymised Data with 3rd Party Disallowed"@en .

ieee-7012-owl:SharingDataNonAnonymisedDisallowed a rdfs:Class,
        owl:Class,
        dpv-owl:Prohibition,
        ieee-7012-owl:DataSharingTerm ;
    dct:created "2024-12-17"^^xsd:date ;
    rdfs:isDefinedBy ieee-7012-owl: ;
    rdfs:subClassOf ieee-7012-owl:SharingDataDisallowed ;
    sw:term_status "accepted"@en ;
    skos:definition "Term that indicates Data Sharing for fully anonymised data is not allowed"@en ;
    skos:prefLabel "Sharing Non-Anonymised Data Disallowed"@en .

ieee-7012-owl:TPR a rdfs:Class,
        owl:Class,
        ieee-7012-owl:Agreement ;
    dct:created "2025-04-09"^^xsd:date ;
    rdfs:isDefinedBy ieee-7012-owl: ;
    rdfs:subClassOf ieee-7012-owl:Agreement ;
    sw:term_status "accepted"@en ;
    skos:definition "Term that indicates the agreement is between two individual humans regarding services, communication, or other activities as mutually agreed within the agreement"@en ;
    skos:prefLabel "Trusted Personal Relationship"@en ;
    dpv-owl:hasObligation ieee-7012-owl:ServiceDeliveryRequired ;
    dpv-owl:hasProhibition ieee-7012-owl:DataSharingDisallowed .

ieee-7012-owl:TPR-IDENTITY-REF a rdfs:Class,
        owl:Class,
        ieee-7012-owl:Agreement ;
    dct:created "2025-04-09"^^xsd:date ;
    rdfs:isDefinedBy ieee-7012-owl: ;
    rdfs:subClassOf ieee-7012-owl:TPR ;
    sw:term_status "accepted"@en ;
    skos:definition "Term that indicates an agreement that establishes the identity of a person through an agreement with another human who validates or vouches for the stated identity as belonging to the associated human"@en ;
    skos:prefLabel "Trusted Personal Relationship - Identity Reference"@en ;
    dpv-owl:hasObligation dpv-owl:IdentityVerification .

ieee-7012-owl:ThirdParty a rdfs:Class,
        owl:Class ;
    dct:created "2024-12-17"^^xsd:date ;
    rdfs:isDefinedBy ieee-7012-owl: ;
    rdfs:subClassOf dpv-owl:LegalEntity ;
    sw:term_status "accepted"@en ;
    skos:definition "A party other than the Person and Entity as first and second parties respectively in the contractual interaction"@en ;
    skos:prefLabel "Third Party"@en .

ieee-7012-owl:Tracking2PAllowed a rdfs:Class,
        owl:Class,
        dpv-owl:Permission,
        ieee-7012-owl:TrackingTerm ;
    dct:created "2024-12-17"^^xsd:date ;
    rdfs:isDefinedBy ieee-7012-owl: ;
    rdfs:subClassOf ieee-7012-owl:TrackingAllowed ;
    sw:term_status "accepted"@en ;
    skos:definition "Term that indicates Tracking 2nd Party is allowed"@en ;
    skos:prefLabel "Tracking by 2nd Party Allowed"@en .

ieee-7012-owl:Tracking3PDisallowed a rdfs:Class,
        owl:Class,
        dpv-owl:Prohibition,
        ieee-7012-owl:TrackingTerm ;
    dct:created "2024-12-17"^^xsd:date ;
    rdfs:isDefinedBy ieee-7012-owl: ;
    rdfs:subClassOf ieee-7012-owl:TrackingDisallowed ;
    sw:term_status "accepted"@en ;
    skos:definition "Term that indicates Tracking 3rd Party is disallowed"@en ;
    skos:prefLabel "Tracking by 3rd Party Disallowed"@en .

ieee-7012-owl:TrackingAllowed a rdfs:Class,
        owl:Class,
        dpv-owl:Permission,
        ieee-7012-owl:TrackingTerm ;
    dct:created "2024-12-17"^^xsd:date ;
    rdfs:isDefinedBy ieee-7012-owl: ;
    rdfs:subClassOf dpv-owl:Permission,
        ieee-7012-owl:TrackingTerm ;
    sw:term_status "accepted"@en ;
    skos:definition "Term that indicates Tracking by 2nd and 3rd parties is allowed"@en ;
    skos:prefLabel "Tracking Allowed"@en .

ieee-7012-owl:TrackingDisallowed a rdfs:Class,
        owl:Class,
        dpv-owl:Prohibition,
        ieee-7012-owl:TrackingTerm ;
    dct:created "2024-12-17"^^xsd:date ;
    rdfs:isDefinedBy ieee-7012-owl: ;
    rdfs:subClassOf dpv-owl:Prohibition,
        ieee-7012-owl:TrackingTerm ;
    sw:term_status "accepted"@en ;
    skos:definition "Term that indicates Tracking by 2nd and 3rd parties is disallowed"@en ;
    skos:prefLabel "Tracking Disallowed"@en .

ieee-7012-owl:TrackingTerm a rdfs:Class,
        owl:Class ;
    dct:created "2024-12-17"^^xsd:date ;
    rdfs:isDefinedBy ieee-7012-owl: ;
    rdfs:subClassOf dpv-owl:ContractualClause ;
    sw:term_status "accepted"@en ;
    skos:definition "Term related to Tracking"@en ;
    skos:prefLabel "Tracking Term"@en .

ieee-7012-owl:TrackingWithFPDisallowed a rdfs:Class,
        owl:Class,
        dpv-owl:Prohibition,
        ieee-7012-owl:TrackingTerm ;
    dct:created "2024-12-17"^^xsd:date ;
    rdfs:isDefinedBy ieee-7012-owl: ;
    rdfs:subClassOf ieee-7012-owl:TrackingDisallowed ;
    sw:term_status "accepted"@en ;
    skos:definition "Term that indicates Tracking involving use of Fingerprinting is not allowed"@en ;
    skos:prefLabel "Tracking With FP Disallowed"@en .

ieee-7012-owl:TrackingWithPIIDisallowed a rdfs:Class,
        owl:Class,
        dpv-owl:Prohibition,
        ieee-7012-owl:TrackingTerm ;
    dct:created "2024-12-17"^^xsd:date ;
    rdfs:isDefinedBy ieee-7012-owl: ;
    rdfs:subClassOf ieee-7012-owl:TrackingDisallowed ;
    sw:term_status "accepted"@en ;
    skos:definition "Term that indicates Tracking involving use of PII is not allowed"@en ;
    skos:prefLabel "Tracking With PII Disallowed"@en .

ieee-7012-owl:TrackingWithoutFPAllowed a rdfs:Class,
        owl:Class,
        dpv-owl:Permission,
        ieee-7012-owl:TrackingTerm ;
    dct:created "2024-12-17"^^xsd:date ;
    rdfs:isDefinedBy ieee-7012-owl: ;
    rdfs:subClassOf ieee-7012-owl:TrackingAllowed ;
    sw:term_status "accepted"@en ;
    skos:definition "Term that indicates Tracking is allowed but only if it does not involve Fingerprinting"@en ;
    skos:prefLabel "Tracking Without FP Allowed"@en .

ieee-7012-owl:TrackingWithoutPIIAllowed a rdfs:Class,
        owl:Class,
        dpv-owl:Permission,
        ieee-7012-owl:TrackingTerm ;
    dct:created "2024-12-17"^^xsd:date ;
    rdfs:isDefinedBy ieee-7012-owl: ;
    rdfs:subClassOf ieee-7012-owl:TrackingAllowed ;
    sw:term_status "accepted"@en ;
    skos:definition "Term that indicates Tracking is allowed but only if it does not use any PII"@en ;
    skos:prefLabel "Tracking Without PII Allowed"@en .

ieee-7012-owl:TransparencyExAnte a rdfs:Class,
        owl:Class,
        dpv-owl:Obligation,
        ieee-7012-owl:TransparencyTerm ;
    dct:created "2024-12-17"^^xsd:date ;
    rdfs:isDefinedBy ieee-7012-owl: ;
    rdfs:subClassOf ieee-7012-owl:TransparencyRequired ;
    sw:term_status "accepted"@en ;
    skos:definition "Term that indicates transparency is obligated ahead of intended process i.e. ex-ante transparency"@en ;
    skos:prefLabel "Transparency Ex Ante"@en .

ieee-7012-owl:TransparencyExPost a rdfs:Class,
        owl:Class,
        dpv-owl:Obligation,
        ieee-7012-owl:TransparencyTerm ;
    dct:created "2024-12-17"^^xsd:date ;
    rdfs:isDefinedBy ieee-7012-owl: ;
    rdfs:subClassOf ieee-7012-owl:TransparencyRequired ;
    sw:term_status "accepted"@en ;
    skos:definition "Term that indicates transparency is obligated after intended process i.e. ex-post transparency"@en ;
    skos:prefLabel "Transparency Ex Post"@en .

ieee-7012-owl:TransparencyNotRequired a rdfs:Class,
        owl:Class,
        ieee-7012-owl:TransparencyTerm ;
    dct:created "2024-12-17"^^xsd:date ;
    rdfs:isDefinedBy ieee-7012-owl: ;
    rdfs:subClassOf ieee-7012-owl:TransparencyRequired ;
    sw:term_status "accepted"@en ;
    skos:definition "Term that indicates transparency is not required to be provided"@en ;
    skos:prefLabel "Transparency Not Required"@en .

ieee-7012-owl:TransparencyOnRequest a rdfs:Class,
        owl:Class,
        dpv-owl:Obligation,
        ieee-7012-owl:TransparencyTerm ;
    dct:created "2024-12-17"^^xsd:date ;
    rdfs:isDefinedBy ieee-7012-owl: ;
    rdfs:subClassOf ieee-7012-owl:TransparencyRequired ;
    sw:term_status "accepted"@en ;
    skos:definition "Term that indicates transparency is obligated upon request"@en ;
    skos:prefLabel "Transparency On Request"@en .

ieee-7012-owl:TransparencyRequired a rdfs:Class,
        owl:Class,
        dpv-owl:Obligation,
        ieee-7012-owl:TransparencyTerm ;
    dct:created "2024-12-17"^^xsd:date ;
    rdfs:isDefinedBy ieee-7012-owl: ;
    rdfs:subClassOf dpv-owl:Obligation,
        ieee-7012-owl:TransparencyTerm ;
    sw:term_status "accepted"@en ;
    skos:definition "Term that indicates transparency is obligated"@en ;
    skos:prefLabel "Transparency Required"@en .

ieee-7012-owl:TransparencyTerm a rdfs:Class,
        owl:Class ;
    dct:created "2024-12-17"^^xsd:date ;
    rdfs:isDefinedBy ieee-7012-owl: ;
    rdfs:subClassOf dpv-owl:ContractualClause ;
    sw:term_status "accepted"@en ;
    skos:definition "Term that indicates transparency as an obligation"@en ;
    skos:prefLabel "Transparency Term"@en .

ieee-7012-owl:hasAgent a rdf:Property,
        owl:ObjectProperty ;
    dcam:rangeIncludes ieee-7012-owl:Agent ;
    dct:created "2024-12-17"^^xsd:date ;
    rdfs:isDefinedBy ieee-7012-owl: ;
    rdfs:subPropertyOf dpv-owl:hasEntity ;
    sw:term_status "accepted"@en ;
    skos:definition "Specifies the agent that represents a party and can act on behalf"@en ;
    skos:prefLabel "has agent"@en ;
    schema:rangeIncludes ieee-7012-owl:Agent .

ieee-7012-owl:hasAgentBehaviour a rdf:Property,
        owl:ObjectProperty ;
    dcam:rangeIncludes ieee-7012-owl:AgentBehaviour ;
    dct:created "2024-12-17"^^xsd:date ;
    rdfs:isDefinedBy ieee-7012-owl: ;
    sw:term_status "accepted"@en ;
    skos:definition "Relation that indicates the behaviour of Privacy Agents"@en ;
    skos:prefLabel "has agent behaviour"@en ;
    schema:rangeIncludes ieee-7012-owl:AgentBehaviour .

ieee-7012-owl:hasAgreement a rdf:Property,
        owl:ObjectProperty ;
    dcam:rangeIncludes ieee-7012-owl:Agreement ;
    dct:created "2024-12-17"^^xsd:date ;
    rdfs:isDefinedBy ieee-7012-owl: ;
    sw:term_status "accepted"@en ;
    skos:definition "Indicates the inclusion or applicability of the specified Privacy Term"@en ;
    skos:prefLabel "has agreement"@en ;
    schema:rangeIncludes ieee-7012-owl:Agreement .

ieee-7012-owl:hasAgreementPreference a rdf:Property,
        owl:ObjectProperty ;
    dcam:rangeIncludes ieee-7012-owl:AgreementPreference ;
    dct:created "2024-12-17"^^xsd:date ;
    rdfs:isDefinedBy ieee-7012-owl: ;
    sw:term_status "accepted"@en ;
    skos:definition "Indicates the inclusion or applicability of the specified Privacy Preference"@en ;
    skos:prefLabel "has privacy preference"@en ;
    schema:rangeIncludes ieee-7012-owl:AgreementPreference .

ieee-7012-owl:hasAgreementRegistry a rdf:Property,
        owl:ObjectProperty ;
    dcam:rangeIncludes ieee-7012-owl:AgreementRegistry ;
    dct:created "2024-12-17"^^xsd:date ;
    rdfs:isDefinedBy ieee-7012-owl: ;
    sw:term_status "accepted"@en ;
    skos:definition "Indicates the inclusion or applicability of the specified Privacy Term Registry"@en ;
    skos:prefLabel "has agreement registry"@en ;
    schema:rangeIncludes ieee-7012-owl:AgreementRegistry .

ieee-7012-owl:hasConflictResolution a rdf:Property,
        owl:ObjectProperty ;
    dcam:rangeIncludes ieee-7012-owl:ConflictResolutionTerm ;
    dct:created "2024-12-17"^^xsd:date ;
    rdfs:isDefinedBy ieee-7012-owl: ;
    sw:term_status "accepted"@en ;
    skos:definition "Relation that indicates the Conflict Resolution Term that should be used"@en ;
    skos:prefLabel "has conflict resolution"@en ;
    schema:rangeIncludes ieee-7012-owl:ConflictResolutionTerm .

ieee-7012-owl:hasDataSharingTerm a rdf:Property,
        owl:ObjectProperty ;
    dcam:rangeIncludes ieee-7012-owl:DataSharingTerm ;
    dct:created "2024-12-17"^^xsd:date ;
    rdfs:isDefinedBy ieee-7012-owl: ;
    sw:term_status "accepted"@en ;
    skos:definition "Relation that associates a Data Sharing Term"@en ;
    skos:prefLabel "has data sharing term"@en ;
    schema:rangeIncludes ieee-7012-owl:DataSharingTerm .

ieee-7012-owl:hasDeonticInterpretation a rdf:Property,
        owl:ObjectProperty ;
    dcam:rangeIncludes ieee-7012-owl:DeonticInterpretationTerm ;
    dct:created "2024-12-17"^^xsd:date ;
    rdfs:isDefinedBy ieee-7012-owl: ;
    sw:term_status "accepted"@en ;
    skos:definition "Relation that indicates the Deontic Interpretation Term that should be used"@en ;
    skos:prefLabel "has deontic interpretation"@en ;
    schema:rangeIncludes ieee-7012-owl:DeonticInterpretationTerm .

ieee-7012-owl:hasEndpoint a rdf:Property,
        owl:ObjectProperty ;
    dcam:rangeIncludes ieee-7012-owl:Endpoint ;
    dct:created "2024-12-17"^^xsd:date ;
    dct:modified "2026-02-03"^^xsd:date ;
    rdfs:isDefinedBy ieee-7012-owl: ;
    sw:term_status "modified"@en ;
    skos:definition "Indicates the endpoint, such as a URL or an address, where 7012 related communications and interactions can be made"@en ;
    skos:prefLabel "has endpoint"@en ;
    schema:rangeIncludes ieee-7012-owl:Endpoint .

ieee-7012-owl:hasFirstParty a rdf:Property,
        owl:ObjectProperty ;
    dcam:rangeIncludes ieee-7012-owl:Person ;
    dct:created "2024-12-17"^^xsd:date ;
    rdfs:isDefinedBy ieee-7012-owl: ;
    rdfs:subPropertyOf dpv-owl:hasEntity ;
    sw:term_status "accepted"@en ;
    skos:definition "Specifies the human individual or Person involved as the first party"@en ;
    skos:prefLabel "has first party"@en ;
    schema:rangeIncludes ieee-7012-owl:Person .

ieee-7012-owl:hasHumanDescription a rdf:Property,
        owl:ObjectProperty ;
    dct:created "2025-04-09"^^xsd:date ;
    rdfs:isDefinedBy ieee-7012-owl: ;
    sw:term_status "accepted"@en ;
    skos:definition "A description intended for humans"@en ;
    skos:prefLabel "has human description"@en .

ieee-7012-owl:hasHumanReadableFormat a rdf:Property,
        owl:ObjectProperty ;
    dcam:rangeIncludes xsd:anyURI ;
    dct:created "2024-12-17"^^xsd:date ;
    rdfs:isDefinedBy ieee-7012-owl: ;
    sw:term_status "accepted"@en ;
    skos:definition "Indicates the specified resource is a human readable format of the subject"@en ;
    skos:prefLabel "has human readable format"@en ;
    schema:rangeIncludes xsd:anyURI .

ieee-7012-owl:hasMachineReadableFormat a rdf:Property,
        owl:ObjectProperty ;
    dcam:rangeIncludes xsd:anyURI ;
    dct:created "2024-12-17"^^xsd:date ;
    rdfs:isDefinedBy ieee-7012-owl: ;
    sw:term_status "accepted"@en ;
    skos:definition "Indicates the specified resource is a machine readable format of the subject"@en ;
    skos:prefLabel "has machine readable format"@en ;
    skos:scopeNote "To assist in interpreting the resource, we strongly suggest using dct:conformsTo with an appropriate URI to indicate the specific standard or specification used to express the resource"@en ;
    schema:rangeIncludes xsd:anyURI .

ieee-7012-owl:hasParty a rdf:Property,
        owl:ObjectProperty ;
    dcam:rangeIncludes ieee-7012-owl:Party ;
    dct:created "2024-12-17"^^xsd:date ;
    rdfs:isDefinedBy ieee-7012-owl: ;
    rdfs:subPropertyOf dpv-owl:hasEntity ;
    sw:term_status "accepted"@en ;
    skos:definition "Specifies that an entity is a party to the context i.e. it has decision making abilities or has obligations and responsibilities"@en ;
    skos:prefLabel "has party"@en ;
    schema:rangeIncludes ieee-7012-owl:Party .

ieee-7012-owl:hasPortabilityTerm a rdf:Property,
        owl:ObjectProperty ;
    dcam:rangeIncludes ieee-7012-owl:PortabilityTerm ;
    dct:created "2024-12-17"^^xsd:date ;
    rdfs:isDefinedBy ieee-7012-owl: ;
    sw:term_status "accepted"@en ;
    skos:definition "Relation that associates a Portability Term"@en ;
    skos:prefLabel "has portability term"@en ;
    schema:rangeIncludes ieee-7012-owl:PortabilityTerm .

ieee-7012-owl:hasPreferenceApplicability a rdf:Property,
        owl:ObjectProperty ;
    dcam:rangeIncludes ieee-7012-owl:PreferenceApplicability ;
    dct:created "2024-12-17"^^xsd:date ;
    rdfs:isDefinedBy ieee-7012-owl: ;
    sw:term_status "accepted"@en ;
    skos:definition "Relation that indicates the applicability of Privacy Preference(s)"@en ;
    skos:prefLabel "has preference applicability"@en ;
    schema:rangeIncludes ieee-7012-owl:PreferenceApplicability .

ieee-7012-owl:hasProfilingTerm a rdf:Property,
        owl:ObjectProperty ;
    dcam:rangeIncludes ieee-7012-owl:ProfilingTerm ;
    dct:created "2024-12-17"^^xsd:date ;
    rdfs:isDefinedBy ieee-7012-owl: ;
    sw:term_status "accepted"@en ;
    skos:definition "Relation that associates a Profiling Term"@en ;
    skos:prefLabel "has profiling term"@en ;
    schema:rangeIncludes ieee-7012-owl:ProfilingTerm .

ieee-7012-owl:hasSecondParty a rdf:Property,
        owl:ObjectProperty ;
    dcam:rangeIncludes ieee-7012-owl:Entity ;
    dct:created "2024-12-17"^^xsd:date ;
    rdfs:isDefinedBy ieee-7012-owl: ;
    rdfs:subPropertyOf dpv-owl:hasEntity ;
    sw:term_status "accepted"@en ;
    skos:definition "Specifies the entity organisation involved as the second party"@en ;
    skos:prefLabel "has second party"@en ;
    schema:rangeIncludes ieee-7012-owl:Entity .

ieee-7012-owl:hasThirdParty a rdf:Property,
        owl:ObjectProperty ;
    dcam:rangeIncludes ieee-7012-owl:ThirdParty ;
    dct:created "2024-12-17"^^xsd:date ;
    rdfs:isDefinedBy ieee-7012-owl: ;
    rdfs:subPropertyOf dpv-owl:hasThirdParty ;
    sw:term_status "accepted"@en ;
    skos:definition "Specifies the a party other than the person or Entity that is involved"@en ;
    skos:prefLabel "has third party"@en ;
    schema:rangeIncludes ieee-7012-owl:ThirdParty .

ieee-7012-owl:hasTrackingTerm a rdf:Property,
        owl:ObjectProperty ;
    dcam:rangeIncludes ieee-7012-owl:TrackingTerm ;
    dct:created "2024-12-17"^^xsd:date ;
    rdfs:isDefinedBy ieee-7012-owl: ;
    sw:term_status "accepted"@en ;
    skos:definition "Relation that associates a Tracking Term"@en ;
    skos:prefLabel "has tracking term"@en ;
    schema:rangeIncludes ieee-7012-owl:TrackingTerm .

ieee-7012-owl:hasTransparencyTerm a rdf:Property,
        owl:ObjectProperty ;
    dcam:rangeIncludes ieee-7012-owl:TransparencyTerm ;
    dct:created "2024-12-17"^^xsd:date ;
    rdfs:isDefinedBy ieee-7012-owl: ;
    sw:term_status "accepted"@en ;
    skos:definition "Relation that associates a Transparency Term"@en ;
    skos:prefLabel "has transparency term"@en ;
    schema:rangeIncludes ieee-7012-owl:TransparencyTerm .

ieee-7012-owl:serialisation-html a profile:ResourceDescriptor ;
    dct:conformsTo <https://www.w3.org/TR/html/> ;
    dct:format <https://www.iana.org/assignments/media-types/text/html> ;
    dct:title "Extension for IEEE 7012 - HTML serialisation" ;
    profile:hasArtifact <https://w3id.org/dpv/standards/ieee/7012/ieee-7012-owl.html> ;
    profile:hasRole role:specification .

ieee-7012-owl:serialisation-jsonld a profile:ResourceDescriptor ;
    dct:conformsTo <https://www.w3.org/TR/json-ld11/> ;
    dct:format <https://www.iana.org/assignments/media-types/application/ld+json> ;
    dct:title "Extension for IEEE 7012 - JSON-LD serialisation" ;
    profile:hasArtifact <https://w3id.org/dpv/standards/ieee/7012/ieee-7012-owl.jsonld> ;
    profile:hasRole role:vocabulary .

ieee-7012-owl:serialisation-n3 a profile:ResourceDescriptor ;
    dct:conformsTo <https://www.w3.org/TeamSubmission/n3/> ;
    dct:format <https://www.iana.org/assignments/media-types/text/n3> ;
    dct:title "Extension for IEEE 7012 - N3 serialisation" ;
    profile:hasArtifact <https://w3id.org/dpv/standards/ieee/7012/ieee-7012-owl.n3> ;
    profile:hasRole role:vocabulary .

ieee-7012-owl:serialisation-rdf a profile:ResourceDescriptor ;
    dct:conformsTo rdf: ;
    dct:format <https://www.iana.org/assignments/media-types/application/rdf+xml> ;
    dct:title "Extension for IEEE 7012 - RDF/XML serialisation" ;
    profile:hasArtifact <https://w3id.org/dpv/standards/ieee/7012/ieee-7012-owl.rdf> ;
    profile:hasRole role:vocabulary .

ieee-7012-owl:serialisation-ttl a profile:ResourceDescriptor ;
    dct:conformsTo <https://www.w3.org/TR/turtle/> ;
    dct:format <https://www.iana.org/assignments/media-types/text/turtle> ;
    dct:title "Extension for IEEE 7012 - Turtle serialisation" ;
    profile:hasArtifact <https://w3id.org/dpv/standards/ieee/7012/ieee-7012-owl.ttl> ;
    profile:hasRole role:vocabulary .

<https://w3id.org/dpv/examples> a profile:ResourceDescriptor ;
    dct:conformsTo <https://www.w3.org/TR/html/> ;
    dct:format <https://www.iana.org/assignments/media-types/text/html> ;
    dct:title "Examples" ;
    profile:hasArtifact <https://w3id.org/dpv/examples> ;
    profile:hasRole role:guidance .

<https://w3id.org/dpv/guides> a profile:ResourceDescriptor ;
    dct:conformsTo <https://www.w3.org/TR/html/> ;
    dct:format <https://www.iana.org/assignments/media-types/text/html> ;
    dct:title "Guides for Data Privacy Vocabulary" ;
    profile:hasArtifact <https://w3id.org/dpv/guides> ;
    profile:hasRole role:guidance .

<https://w3id.org/dpv/primer> a profile:ResourceDescriptor ;
    dct:conformsTo <https://www.w3.org/TR/html/> ;
    dct:format <https://www.iana.org/assignments/media-types/text/html> ;
    dct:title "Primer for Data Privacy Vocabulary" ;
    profile:hasArtifact <https://w3id.org/dpv/primer> ;
    profile:hasRole role:guidance .

ieee-7012-owl: a owl:Ontology,
        profile:Profile ;
    dct:bibliographicCitation "Harshvardhan J. Pandit, Beatriz Esteves, Georg P. Krog, Paul Ryan, Delaram Golpayegani, Julian Flake (2025) Data Privacy Vocabulary (DPV)  Version 2.0. In: Demartini, G., et al. The Semantic Web  ISWC 2024. ISWC 2024. Lecture Notes in Computer Science, vol 15233. Springer, Cham. https://doi.org/10.1007/978-3-031-77847-6_10" ;
    dct:conformsTo <http://www.w3.org/2002/07/owl>,
        "http://www.w3.org/2000/01/rdf-schema",
        "http://www.w3.org/2004/02/skos/core" ;
    dct:created "2025-01-12"@en ;
    dct:creator [ a dct:Agent,
                foaf:Person ;
            scoro:hasORCID "0000-0003-0259-7560" ;
            org:memberOf [ a foaf:Organization ;
                    foaf:name "IDLab, IMEC, Ghent University" ] ;
            foaf:homepage "https://w3id.org/people/besteves" ;
            foaf:name "Beatriz Esteves" ],
        [ a dct:Agent,
                foaf:Person ;
            scoro:hasORCID "0000-0002-5068-3714" ;
            org:memberOf [ a foaf:Organization ;
                    foaf:name "AI Accountability Lab (AIAL), Trinity College Dublin" ] ;
            foaf:homepage "https://harshp.com/" ;
            foaf:name "Harshvardhan J. Pandit" ],
        [ a dct:Agent,
                foaf:Person ;
            org:memberOf [ a foaf:Organization ;
                    foaf:name "JLINC Labs" ] ;
            foaf:name "Iain Henderson" ] ;
    dct:description "Extension to the Data Privacy Vocabulary (DPV) providing concepts for implementing IEEE 7012"@en ;
    dct:hasVersion ieee-7012-owl: ;
    dct:identifier "https://w3id.org/dpv/standards/ieee/7012" ;
    dct:issued "2025-01-12"@en ;
    dct:license <https://www.w3.org/copyright/document-license-2023/> ;
    dct:modified "2026-02-25"@en ;
    dct:publisher <https://www.w3.org/> ;
    dct:source <https://www.w3.org/groups/cg/dpvcg/> ;
    dct:title "Extension for IEEE 7012"@en ;
    bibo:doi "10.5281/zenodo.12505841" ;
    bibo:status "http://purl.org/ontology/bibo/status/draft" ;
    vann:preferredNamespacePrefix "ieee-7012" ;
    vann:preferredNamespaceUri "https://w3id.org/dpv/standards/ieee/7012#" ;
    rdfs:Label "IEEE-7012"@en ;
    owl:versionIRI <https://w3id.org/dpv/2.3/standards/ieee/7012/owl#> ;
    owl:versionInfo "2.3" ;
    profile:hasResource <https://w3id.org/dpv/examples>,
        <https://w3id.org/dpv/guides>,
        <https://w3id.org/dpv/primer>,
        ieee-7012-owl:serialisation-html,
        ieee-7012-owl:serialisation-jsonld,
        ieee-7012-owl:serialisation-n3,
        ieee-7012-owl:serialisation-rdf,
        ieee-7012-owl:serialisation-ttl ;
    profile:isProfileOf <http://www.w3.org/2002/07/owl>,
        <https://w3id.org/dpv/owl>,
        ieee-7012-owl: ;
    foaf:logo <https://w3id.org/dpv/media/logo.png> ;
    schema:version "2.3" .

