@prefix bibo: <http://purl.org/ontology/bibo/> .
@prefix dct: <http://purl.org/dc/terms/> .
@prefix dpv: <https://w3id.org/dpv#> .
@prefix foaf: <http://xmlns.com/foaf/0.1/> .
@prefix org: <http://www.w3.org/ns/org#> .
@prefix owl: <http://www.w3.org/2002/07/owl#> .
@prefix profile: <http://www.w3.org/ns/dx/prof/> .
@prefix rdfs: <http://www.w3.org/2000/01/rdf-schema#> .
@prefix role: <http://www.w3.org/ns/dx/prof/role/> .
@prefix schema: <https://schema.org/> .
@prefix scoro: <http://purl.org/spar/scoro/> .
@prefix sector-health: <https://w3id.org/dpv/sector/health#> .
@prefix skos: <http://www.w3.org/2004/02/skos/core#> .
@prefix sw: <http://www.w3.org/2003/06/sw-vocab-status/ns#> .
@prefix vann: <http://purl.org/vocab/vann/> .
@prefix xsd: <http://www.w3.org/2001/XMLSchema#> .

sector-health:CompatibilityUnknown a rdfs:Class,
        skos:Concept,
        sector-health:ReuseCompatibility ;
    dct:contributor _:person-arthit-suriyawongkul,
        _:person-beatriz-esteves,
        _:person-delaram-golpayegani,
        _:person-georg-p-krog,
        _:person-harshvardhan-j-pandit,
        _:person-julian-flake ;
    dct:created "2025-06-19"^^xsd:date ;
    rdfs:isDefinedBy sector-health: ;
    sw:term_status "accepted"@en ;
    skos:broader dpv:CompatibilityUnknown ;
    skos:definition "Status indicating the compatibility for reuse of health data for the context is currently unknown"@en ;
    skos:inScheme sector-health:status-classes ;
    skos:prefLabel "Compatibility Unknown"@en .

sector-health:PrimaryUse a rdfs:Class,
        skos:Concept,
        sector-health:ReuseCompatibility ;
    dct:contributor _:person-arthit-suriyawongkul,
        _:person-beatriz-esteves,
        _:person-delaram-golpayegani,
        _:person-georg-p-krog,
        _:person-harshvardhan-j-pandit,
        _:person-julian-flake ;
    dct:created "2025-06-19"^^xsd:date ;
    rdfs:isDefinedBy sector-health: ;
    sw:term_status "accepted"@en ;
    skos:broader dpv:PrimaryUse ;
    skos:definition "Status indicating the reuse of health is compatible with the original purpose or use i.e. it can be considered as 'Primary Use'"@en ;
    skos:inScheme sector-health:status-classes ;
    skos:prefLabel "Primary Use"@en ;
    skos:scopeNote "Primary Use refers to an assessment where two contexts are found to be compatible, e.g. if purpose is used to test compatibility, then for two activities the second activity is said be the primary use if its purpose is compatible with the first activity's purpose"@en .

sector-health:ReuseCompatibility a rdfs:Class,
        skos:Concept ;
    dct:contributor _:person-arthit-suriyawongkul,
        _:person-beatriz-esteves,
        _:person-delaram-golpayegani,
        _:person-georg-p-krog,
        _:person-harshvardhan-j-pandit,
        _:person-julian-flake ;
    dct:created "2025-06-19"^^xsd:date ;
    rdfs:isDefinedBy sector-health: ;
    rdfs:subClassOf dpv:ReuseCompatibility ;
    sw:term_status "accepted"@en ;
    skos:broader dpv:ReuseCompatibility ;
    skos:definition "Status indicating whether the reuse of health data is compatible for given context"@en ;
    skos:inScheme sector-health:status-classes ;
    skos:prefLabel "ReuseCompatibility"@en ;
    skos:scopeNote "Compatibility refers to whether two contexts, such as dpv:Process instances, are compatible with each other based on a criteria which is not defined by the concept. This criteria can be based on requirements from law, such as GDPR's purpose compatibility or can be based on privacy norms such as contextual integrity. To express such interpretations, further concepts should be expanded from this base concept"@en .

sector-health:SecondaryUse a rdfs:Class,
        skos:Concept,
        sector-health:ReuseCompatibility ;
    dct:contributor _:person-arthit-suriyawongkul,
        _:person-beatriz-esteves,
        _:person-delaram-golpayegani,
        _:person-georg-p-krog,
        _:person-harshvardhan-j-pandit,
        _:person-julian-flake ;
    dct:created "2025-06-19"^^xsd:date ;
    rdfs:isDefinedBy sector-health: ;
    sw:term_status "accepted"@en ;
    skos:broader dpv:SecondaryUse ;
    skos:definition "Status indicating the reuse of health is incompatible with the original purpose or use i.e. it is considered as 'Secondary Use'"@en ;
    skos:inScheme sector-health:status-classes ;
    skos:prefLabel "Secondary Use"@en ;
    skos:scopeNote "Secondary Use refers to an assessment where two contexts are found to be incompatible, e.g. if purpose is used to test compatibility, then for two activities the second activity is said be the secondary use if its purpose is incompatible with the first activity's purpose"@en .

<https://w3id.org/dpv/sector/health> a owl:Ontology,
        profile:Profile ;
    dct:bibliographicCitation "Harshvardhan J. Pandit, Beatriz Esteves, Georg P. Krog, Paul Ryan, Delaram Golpayegani, Julian Flake (2025) Data Privacy Vocabulary (DPV) – Version 2.0. In: Demartini, G., et al. The Semantic Web – ISWC 2024. ISWC 2024. Lecture Notes in Computer Science, vol 15233. Springer, Cham. https://doi.org/10.1007/978-3-031-77847-6_10" ;
    dct:conformsTo "http://www.w3.org/2000/01/rdf-schema",
        "http://www.w3.org/2004/02/skos/core" ;
    dct:contributor _:person-arthit-suriyawongkul,
        _:person-beatriz-esteves,
        _:person-delaram-golpayegani,
        _:person-georg-p-krog,
        _:person-harshvardhan-j-pandit,
        _:person-julian-flake ;
    dct:created "2024-12-01"@en ;
    dct:creator _:person-beatriz-esteves,
        _:person-harshvardhan-j-pandit,
        _:person-julian-flake ;
    dct:description "Extension to the Data Privacy Vocabulary (DPV) providing concepts for the health sector"@en ;
    dct:identifier "https://w3id.org/dpv/sector/health" ;
    dct:issued "2024-12-01"@en ;
    dct:license <https://www.w3.org/copyright/document-license-2023/> ;
    dct:modified "2026-02-25"@en ;
    dct:publisher <https://www.w3.org/> ;
    dct:source <https://www.w3.org/groups/cg/dpvcg/> ;
    dct:title "Health Sector Concepts"@en ;
    bibo:doi "10.5281/zenodo.12505841" ;
    bibo:status "http://purl.org/ontology/bibo/status/draft" ;
    vann:preferredNamespacePrefix "sector-health" ;
    vann:preferredNamespaceUri "https://w3id.org/dpv/sector/health#" ;
    rdfs:Label "SECTOR-HEALTH"@en ;
    owl:versionIRI <https://w3id.org/dpv/2.3/sector/health> ;
    owl:versionInfo "2.3" ;
    profile:hasResource <https://w3id.org/dpv/examples>,
        <https://w3id.org/dpv/guides>,
        <https://w3id.org/dpv/primer>,
        sector-health:serialisation-html,
        sector-health:serialisation-ttl ;
    profile:isProfileOf rdfs:,
        skos:,
        <https://w3id.org/dpv> ;
    foaf:logo <https://w3id.org/dpv/media/logo.png> ;
    schema:version "2.3" .

sector-health:serialisation-html a profile:ResourceDescriptor ;
    dct:conformsTo <https://www.w3.org/TR/html/> ;
    dct:format <https://www.iana.org/assignments/media-types/text/html> ;
    dct:title "Health Sector Concepts - HTML serialisation" ;
    profile:hasArtifact <https://w3id.org/dpv/sector/health/sector-health.html> ;
    profile:hasRole role:specification .

sector-health:serialisation-ttl a profile:ResourceDescriptor ;
    dct:conformsTo <https://www.w3.org/TR/turtle/> ;
    dct:format <https://www.iana.org/assignments/media-types/text/turtle> ;
    dct:title "Health Sector Concepts - Turtle serialisation" ;
    profile:hasArtifact <https://w3id.org/dpv/sector/health/sector-health.ttl> ;
    profile:hasRole role:vocabulary .

<https://w3id.org/dpv/examples> a profile:ResourceDescriptor ;
    dct:conformsTo <https://www.w3.org/TR/html/> ;
    dct:format <https://www.iana.org/assignments/media-types/text/html> ;
    dct:title "Examples" ;
    profile:hasArtifact <https://w3id.org/dpv/examples> ;
    profile:hasRole role:guidance .

<https://w3id.org/dpv/guides> a profile:ResourceDescriptor ;
    dct:conformsTo <https://www.w3.org/TR/html/> ;
    dct:format <https://www.iana.org/assignments/media-types/text/html> ;
    dct:title "Guides for Data Privacy Vocabulary" ;
    profile:hasArtifact <https://w3id.org/dpv/guides> ;
    profile:hasRole role:guidance .

<https://w3id.org/dpv/primer> a profile:ResourceDescriptor ;
    dct:conformsTo <https://www.w3.org/TR/html/> ;
    dct:format <https://www.iana.org/assignments/media-types/text/html> ;
    dct:title "Primer for Data Privacy Vocabulary" ;
    profile:hasArtifact <https://w3id.org/dpv/primer> ;
    profile:hasRole role:guidance .

sector-health:status-classes a skos:ConceptScheme .

_:org-ai-accountability-lab-aial-trinity-college-dublin a foaf:Organization ;
    foaf:name "AI Accountability Lab (AIAL), Trinity College Dublin" .

_:org-idlab-imec-ghent-university a foaf:Organization ;
    foaf:name "IDLab, IMEC, Ghent University" .

_:org-signatu-as a foaf:Organization ;
    foaf:name "Signatu AS" .

_:org-university-of-koblenz a foaf:Organization ;
    foaf:name "University of Koblenz" .

_:org-adapt-centre-trinity-college-dublin a foaf:Organization ;
    foaf:name "ADAPT Centre, Trinity College Dublin" .

_:person-arthit-suriyawongkul a dct:Agent,
        foaf:Person ;
    scoro:hasORCID "0000-0002-9698-1899" ;
    org:memberOf _:org-adapt-centre-trinity-college-dublin ;
    foaf:name "Arthit Suriyawongkul" .

_:person-delaram-golpayegani a dct:Agent,
        foaf:Person ;
    scoro:hasORCID "0000-0002-1208-186X" ;
    org:memberOf _:org-adapt-centre-trinity-college-dublin ;
    foaf:name "Delaram Golpayegani" .

_:person-georg-p-krog a dct:Agent,
        foaf:Person ;
    org:memberOf _:org-signatu-as ;
    foaf:homepage "https://www.linkedin.com/in/georg-philip-krog-a2a278104/" ;
    foaf:name "Georg P. Krog" .

_:person-beatriz-esteves a dct:Agent,
        foaf:Person ;
    scoro:hasORCID "0000-0003-0259-7560" ;
    org:memberOf _:org-idlab-imec-ghent-university ;
    foaf:homepage "https://w3id.org/people/besteves" ;
    foaf:name "Beatriz Esteves" .

_:person-harshvardhan-j-pandit a dct:Agent,
        foaf:Person ;
    scoro:hasORCID "0000-0002-5068-3714" ;
    org:memberOf _:org-ai-accountability-lab-aial-trinity-college-dublin ;
    foaf:homepage "https://harshp.com/" ;
    foaf:name "Harshvardhan J. Pandit" .

_:person-julian-flake a dct:Agent,
        foaf:Person ;
    scoro:hasORCID "0009-0006-4623-1463" ;
    org:memberOf _:org-university-of-koblenz ;
    foaf:name "Julian Flake" .

