<?xml version="1.0" encoding="utf-8"?>
<rdf:RDF
   xmlns:bibo="http://purl.org/ontology/bibo/"
   xmlns:dct="http://purl.org/dc/terms/"
   xmlns:foaf="http://xmlns.com/foaf/0.1/"
   xmlns:org="http://www.w3.org/ns/org#"
   xmlns:owl="http://www.w3.org/2002/07/owl#"
   xmlns:profile="http://www.w3.org/ns/dx/prof/"
   xmlns:rdf="http://www.w3.org/1999/02/22-rdf-syntax-ns#"
   xmlns:rdfs="http://www.w3.org/2000/01/rdf-schema#"
   xmlns:schema="https://schema.org/"
   xmlns:scoro="http://purl.org/spar/scoro/"
   xmlns:skos="http://www.w3.org/2004/02/skos/core#"
   xmlns:sw="http://www.w3.org/2003/06/sw-vocab-status/ns#"
   xmlns:vann="http://purl.org/vocab/vann/"
>
  <rdf:Description rdf:about="https://w3id.org/dpv/sector/health/owl#serialisation-jsonld">
    <dct:title>Health Sector Concepts - JSON-LD serialisation</dct:title>
    <dct:conformsTo rdf:resource="https://www.w3.org/TR/json-ld11/"/>
    <profile:hasArtifact rdf:resource="https://w3id.org/dpv/sector/health/sector-health-owl.jsonld"/>
    <rdf:type rdf:resource="http://www.w3.org/ns/dx/prof/ResourceDescriptor"/>
    <dct:format rdf:resource="https://www.iana.org/assignments/media-types/application/ld+json"/>
    <profile:hasRole rdf:resource="http://www.w3.org/ns/dx/prof/role/vocabulary"/>
  </rdf:Description>
  <rdf:Description rdf:about="https://w3id.org/dpv/sector/health/owl#">
    <owl:versionIRI rdf:resource="https://w3id.org/dpv/2.3/sector/health/owl#"/>
    <profile:hasResource rdf:resource="https://w3id.org/dpv/sector/health/owl#serialisation-n3"/>
    <profile:hasResource rdf:resource="https://w3id.org/dpv/guides"/>
    <profile:hasResource rdf:resource="https://w3id.org/dpv/sector/health/owl#serialisation-jsonld"/>
    <profile:hasResource rdf:resource="https://w3id.org/dpv/sector/health/owl#serialisation-ttl"/>
    <profile:hasResource rdf:resource="https://w3id.org/dpv/examples"/>
    <profile:hasResource rdf:resource="https://w3id.org/dpv/sector/health/owl#serialisation-rdf"/>
    <profile:hasResource rdf:resource="https://w3id.org/dpv/sector/health/owl#serialisation-html"/>
    <profile:hasResource rdf:resource="https://w3id.org/dpv/primer"/>
    <dct:conformsTo>http://www.w3.org/2004/02/skos/core</dct:conformsTo>
    <dct:conformsTo rdf:resource="http://www.w3.org/2002/07/owl"/>
    <dct:conformsTo>http://www.w3.org/2000/01/rdf-schema</dct:conformsTo>
    <dct:issued xml:lang="en">2024-12-01</dct:issued>
    <dct:description xml:lang="en">Extension to the Data Privacy Vocabulary (DPV) providing concepts for the health sector</dct:description>
    <vann:preferredNamespaceUri>https://w3id.org/dpv/sector/health#</vann:preferredNamespaceUri>
    <dct:creator rdf:nodeID="person-julian-flake"/>
    <dct:creator rdf:nodeID="person-harshvardhan-j-pandit"/>
    <dct:creator rdf:nodeID="person-beatriz-esteves"/>
    <dct:source rdf:resource="https://www.w3.org/groups/cg/dpvcg/"/>
    <dct:created xml:lang="en">2024-12-01</dct:created>
    <profile:isProfileOf rdf:resource="https://w3id.org/dpv/owl"/>
    <profile:isProfileOf rdf:resource="http://www.w3.org/2002/07/owl"/>
    <profile:isProfileOf rdf:resource="https://w3id.org/dpv/sector/health/owl#"/>
    <rdf:type rdf:resource="http://www.w3.org/2002/07/owl#Ontology"/>
    <rdf:type rdf:resource="http://www.w3.org/ns/dx/prof/Profile"/>
    <rdfs:Label xml:lang="en">SECTOR-HEALTH</rdfs:Label>
    <schema:version>2.3</schema:version>
    <foaf:logo rdf:resource="https://w3id.org/dpv/media/logo.png"/>
    <bibo:status>http://purl.org/ontology/bibo/status/draft</bibo:status>
    <dct:publisher rdf:resource="https://www.w3.org/"/>
    <dct:license rdf:resource="https://www.w3.org/copyright/document-license-2023/"/>
    <dct:modified xml:lang="en">2026-02-25</dct:modified>
    <dct:contributor rdf:nodeID="person-beatriz-esteves"/>
    <dct:hasVersion rdf:resource="https://w3id.org/dpv/sector/health/owl#"/>
    <vann:preferredNamespacePrefix>sector-health</vann:preferredNamespacePrefix>
    <bibo:doi>10.5281/zenodo.12505841</bibo:doi>
    <dct:bibliographicCitation>Harshvardhan J. Pandit, Beatriz Esteves, Georg P. Krog, Paul Ryan, Delaram Golpayegani, Julian Flake (2025) Data Privacy Vocabulary (DPV) – Version 2.0. In: Demartini, G., et al. The Semantic Web – ISWC 2024. ISWC 2024. Lecture Notes in Computer Science, vol 15233. Springer, Cham. https://doi.org/10.1007/978-3-031-77847-6_10</dct:bibliographicCitation>
    <dct:title xml:lang="en">Health Sector Concepts</dct:title>
    <dct:identifier>https://w3id.org/dpv/sector/health</dct:identifier>
    <owl:versionInfo>2.3</owl:versionInfo>
  </rdf:Description>
  <rdf:Description rdf:about="https://w3id.org/dpv/sector/health/owl#InteroperabilitySoftwareForEHRSystem">
    <rdfs:isDefinedBy rdf:resource="https://w3id.org/dpv/sector/health/owl#"/>
    <rdf:type rdf:resource="https://w3id.org/dpv/owl#Technology"/>
    <rdf:type rdf:resource="http://www.w3.org/2000/01/rdf-schema#Class"/>
    <rdf:type rdf:resource="http://www.w3.org/2002/07/owl#Class"/>
    <dct:contributor rdf:nodeID="person-beatriz-esteves"/>
    <dct:created rdf:datatype="http://www.w3.org/2001/XMLSchema#date">2025-10-28</dct:created>
    <skos:definition xml:lang="en">Software component of the EHR system which provides and receives personal electronic health data under a priority category for primary use established under the EHDS Regulation in the European electronic health record exchange format</skos:definition>
    <skos:prefLabel xml:lang="en">Interoperability Software for EHR System</skos:prefLabel>
    <sw:term_status xml:lang="en">accepted</sw:term_status>
    <rdfs:subClassOf rdf:resource="https://w3id.org/dpv/tech/owl#Software"/>
  </rdf:Description>
  <rdf:Description rdf:about="https://w3id.org/dpv/sector/health/owl#serialisation-rdf">
    <profile:hasArtifact rdf:resource="https://w3id.org/dpv/sector/health/sector-health-owl.rdf"/>
    <rdf:type rdf:resource="http://www.w3.org/ns/dx/prof/ResourceDescriptor"/>
    <dct:title>Health Sector Concepts - RDF/XML serialisation</dct:title>
    <profile:hasRole rdf:resource="http://www.w3.org/ns/dx/prof/role/vocabulary"/>
    <dct:format rdf:resource="https://www.iana.org/assignments/media-types/application/rdf+xml"/>
    <dct:conformsTo rdf:resource="http://www.w3.org/1999/02/22-rdf-syntax-ns#"/>
  </rdf:Description>
  <rdf:Description rdf:about="https://w3id.org/dpv/sector/health/owl#System">
    <rdf:type rdf:resource="https://w3id.org/dpv/owl#Technology"/>
    <rdf:type rdf:resource="http://www.w3.org/2000/01/rdf-schema#Class"/>
    <rdf:type rdf:resource="http://www.w3.org/2002/07/owl#Class"/>
    <dct:contributor rdf:nodeID="person-beatriz-esteves"/>
    <dct:created rdf:datatype="http://www.w3.org/2001/XMLSchema#date">2025-10-28</dct:created>
    <skos:definition xml:lang="en">A system whereby the software and/or hardware allows personal electronic health data to be collected and processed, to be used by healthcare providers when providing patient care or by patients when accessing their electronic health data</skos:definition>
    <skos:prefLabel xml:lang="en">Electronic Health Record System</skos:prefLabel>
    <rdfs:isDefinedBy rdf:resource="https://w3id.org/dpv/sector/health/owl#"/>
    <sw:term_status xml:lang="en">accepted</sw:term_status>
    <rdfs:subClassOf rdf:resource="https://w3id.org/dpv/tech/owl#System"/>
  </rdf:Description>
  <rdf:Description rdf:about="https://w3id.org/dpv/sector/health/owl#EHRSystem">
    <skos:definition xml:lang="en">A system whereby the software and/or hardware allows electronic health record data to be collected and processed, to be used by healthcare providers when providing patient care or by patients when accessing their electronic health data</skos:definition>
    <rdf:type rdf:resource="http://www.w3.org/2000/01/rdf-schema#Class"/>
    <rdf:type rdf:resource="https://w3id.org/dpv/owl#Technology"/>
    <rdf:type rdf:resource="http://www.w3.org/2002/07/owl#Class"/>
    <sw:term_status xml:lang="en">accepted</sw:term_status>
    <rdfs:isDefinedBy rdf:resource="https://w3id.org/dpv/sector/health/owl#"/>
    <dct:contributor rdf:nodeID="person-beatriz-esteves"/>
    <dct:created rdf:datatype="http://www.w3.org/2001/XMLSchema#date">2025-10-28</dct:created>
    <skos:prefLabel xml:lang="en">Electronic Health Record System</skos:prefLabel>
    <rdfs:subClassOf rdf:resource="https://w3id.org/dpv/sector/health/owl#System"/>
  </rdf:Description>
  <rdf:Description rdf:about="https://w3id.org/dpv/examples">
    <profile:hasArtifact rdf:resource="https://w3id.org/dpv/examples"/>
    <dct:format rdf:resource="https://www.iana.org/assignments/media-types/text/html"/>
    <profile:hasRole rdf:resource="http://www.w3.org/ns/dx/prof/role/guidance"/>
    <dct:title>Examples</dct:title>
    <dct:conformsTo rdf:resource="https://www.w3.org/TR/html/"/>
    <rdf:type rdf:resource="http://www.w3.org/ns/dx/prof/ResourceDescriptor"/>
  </rdf:Description>
  <rdf:Description rdf:about="https://w3id.org/dpv/sector/health/owl#WellnessApplication">
    <rdfs:isDefinedBy rdf:resource="https://w3id.org/dpv/sector/health/owl#"/>
    <dct:contributor rdf:nodeID="person-beatriz-esteves"/>
    <dct:created rdf:datatype="http://www.w3.org/2001/XMLSchema#date">2025-10-28</dct:created>
    <rdf:type rdf:resource="https://w3id.org/dpv/owl#Technology"/>
    <rdf:type rdf:resource="http://www.w3.org/2000/01/rdf-schema#Class"/>
    <rdf:type rdf:resource="http://www.w3.org/2002/07/owl#Class"/>
    <skos:prefLabel xml:lang="en">Wellness Application</skos:prefLabel>
    <sw:term_status xml:lang="en">accepted</sw:term_status>
    <skos:definition xml:lang="en">Software component for the processing of electronic health data originating from wellness applications</skos:definition>
    <rdfs:subClassOf rdf:resource="https://w3id.org/dpv/sector/health/owl#HealthApplication"/>
  </rdf:Description>
  <rdf:Description rdf:about="https://w3id.org/dpv/sector/health/owl#ElectronicHealthDataAccessService">
    <rdf:type rdf:resource="http://www.w3.org/2000/01/rdf-schema#Class"/>
    <rdf:type rdf:resource="https://w3id.org/dpv/owl#Technology"/>
    <rdf:type rdf:resource="http://www.w3.org/2002/07/owl#Class"/>
    <rdfs:isDefinedBy rdf:resource="https://w3id.org/dpv/sector/health/owl#"/>
    <dct:contributor rdf:nodeID="person-beatriz-esteves"/>
    <dct:created rdf:datatype="http://www.w3.org/2001/XMLSchema#date">2025-10-28</dct:created>
    <skos:prefLabel xml:lang="en">Electronic Health Data Access Service</skos:prefLabel>
    <skos:definition xml:lang="en">Technical service, such as an online portal or application, that allows data subjects to access their electronic health data or the electronic health data of those natural persons whose electronic health data they are legally authorised to access</skos:definition>
    <sw:term_status xml:lang="en">accepted</sw:term_status>
    <rdfs:subClassOf rdf:resource="https://w3id.org/dpv/tech/owl#Service"/>
  </rdf:Description>
  <rdf:Description rdf:about="https://w3id.org/dpv/sector/health/owl#LoggingSoftwareForEHRSystem">
    <skos:prefLabel xml:lang="en">Logging Software for EHR System</skos:prefLabel>
    <sw:term_status xml:lang="en">accepted</sw:term_status>
    <rdf:type rdf:resource="http://www.w3.org/2000/01/rdf-schema#Class"/>
    <rdf:type rdf:resource="https://w3id.org/dpv/owl#Technology"/>
    <rdf:type rdf:resource="http://www.w3.org/2002/07/owl#Class"/>
    <skos:definition xml:lang="en">Software component of the EHR system which provides logging information related to access by health professionals or other individuals to priority categories of personal electronic health data</skos:definition>
    <dct:contributor rdf:nodeID="person-beatriz-esteves"/>
    <dct:created rdf:datatype="http://www.w3.org/2001/XMLSchema#date">2025-10-28</dct:created>
    <rdfs:isDefinedBy rdf:resource="https://w3id.org/dpv/sector/health/owl#"/>
    <rdfs:subClassOf rdf:resource="https://w3id.org/dpv/tech/owl#Software"/>
  </rdf:Description>
  <rdf:Description rdf:nodeID="org-university-of-koblenz">
    <foaf:name>University of Koblenz</foaf:name>
    <rdf:type rdf:resource="http://xmlns.com/foaf/0.1/Organization"/>
  </rdf:Description>
  <rdf:Description rdf:nodeID="person-beatriz-esteves">
    <scoro:hasORCID>0000-0003-0259-7560</scoro:hasORCID>
    <rdf:type rdf:resource="http://purl.org/dc/terms/Agent"/>
    <rdf:type rdf:resource="http://xmlns.com/foaf/0.1/Person"/>
    <org:memberOf rdf:nodeID="org-idlab-imec-ghent-university"/>
    <foaf:name>Beatriz Esteves</foaf:name>
    <foaf:homepage>https://w3id.org/people/besteves</foaf:homepage>
  </rdf:Description>
  <rdf:Description rdf:about="https://w3id.org/dpv/sector/health/owl#HealthApplication">
    <rdf:type rdf:resource="https://w3id.org/dpv/owl#Technology"/>
    <rdf:type rdf:resource="http://www.w3.org/2000/01/rdf-schema#Class"/>
    <rdf:type rdf:resource="http://www.w3.org/2002/07/owl#Class"/>
    <dct:contributor rdf:nodeID="person-beatriz-esteves"/>
    <dct:created rdf:datatype="http://www.w3.org/2001/XMLSchema#date">2025-10-28</dct:created>
    <sw:term_status xml:lang="en">accepted</sw:term_status>
    <skos:prefLabel xml:lang="en">Health Application</skos:prefLabel>
    <rdfs:isDefinedBy rdf:resource="https://w3id.org/dpv/sector/health/owl#"/>
    <skos:definition xml:lang="en">Software component for the processing of electronic health data, specifically for providing information on the health of natural persons, or the delivery of care for purposes other than the provision of healthcare</skos:definition>
    <rdfs:subClassOf rdf:resource="https://w3id.org/dpv/tech/owl#Application"/>
  </rdf:Description>
  <rdf:Description rdf:nodeID="person-harshvardhan-j-pandit">
    <scoro:hasORCID>0000-0002-5068-3714</scoro:hasORCID>
    <rdf:type rdf:resource="http://purl.org/dc/terms/Agent"/>
    <rdf:type rdf:resource="http://xmlns.com/foaf/0.1/Person"/>
    <org:memberOf rdf:nodeID="org-ai-accountability-lab-aial-trinity-college-dublin"/>
    <foaf:homepage>https://harshp.com/</foaf:homepage>
    <foaf:name>Harshvardhan J. Pandit</foaf:name>
  </rdf:Description>
  <rdf:Description rdf:about="https://w3id.org/dpv/sector/health/owl#serialisation-n3">
    <dct:title>Health Sector Concepts - N3 serialisation</dct:title>
    <dct:conformsTo rdf:resource="https://www.w3.org/TeamSubmission/n3/"/>
    <rdf:type rdf:resource="http://www.w3.org/ns/dx/prof/ResourceDescriptor"/>
    <profile:hasArtifact rdf:resource="https://w3id.org/dpv/sector/health/sector-health-owl.n3"/>
    <dct:format rdf:resource="https://www.iana.org/assignments/media-types/text/n3"/>
    <profile:hasRole rdf:resource="http://www.w3.org/ns/dx/prof/role/vocabulary"/>
  </rdf:Description>
  <rdf:Description rdf:about="https://w3id.org/dpv/sector/health/owl#serialisation-ttl">
    <profile:hasRole rdf:resource="http://www.w3.org/ns/dx/prof/role/vocabulary"/>
    <profile:hasArtifact rdf:resource="https://w3id.org/dpv/sector/health/sector-health-owl.ttl"/>
    <dct:conformsTo rdf:resource="https://www.w3.org/TR/turtle/"/>
    <dct:format rdf:resource="https://www.iana.org/assignments/media-types/text/turtle"/>
    <dct:title>Health Sector Concepts - Turtle serialisation</dct:title>
    <rdf:type rdf:resource="http://www.w3.org/ns/dx/prof/ResourceDescriptor"/>
  </rdf:Description>
  <rdf:Description rdf:nodeID="org-idlab-imec-ghent-university">
    <rdf:type rdf:resource="http://xmlns.com/foaf/0.1/Organization"/>
    <foaf:name>IDLab, IMEC, Ghent University</foaf:name>
  </rdf:Description>
  <rdf:Description rdf:about="https://w3id.org/dpv/sector/health/owl#HealthProfessionalAccessService">
    <skos:definition xml:lang="en">Technical service, supported by an EHR system, that enables health professionals to access data of natural persons under their care</skos:definition>
    <sw:term_status xml:lang="en">accepted</sw:term_status>
    <rdf:type rdf:resource="http://www.w3.org/2000/01/rdf-schema#Class"/>
    <rdf:type rdf:resource="https://w3id.org/dpv/owl#Technology"/>
    <rdf:type rdf:resource="http://www.w3.org/2002/07/owl#Class"/>
    <rdfs:isDefinedBy rdf:resource="https://w3id.org/dpv/sector/health/owl#"/>
    <dct:contributor rdf:nodeID="person-beatriz-esteves"/>
    <dct:created rdf:datatype="http://www.w3.org/2001/XMLSchema#date">2025-10-28</dct:created>
    <skos:prefLabel xml:lang="en">Health Professional Access Service</skos:prefLabel>
    <rdfs:subClassOf rdf:resource="https://w3id.org/dpv/tech/owl#Service"/>
  </rdf:Description>
  <rdf:Description rdf:about="https://w3id.org/dpv/guides">
    <profile:hasArtifact rdf:resource="https://w3id.org/dpv/guides"/>
    <dct:format rdf:resource="https://www.iana.org/assignments/media-types/text/html"/>
    <profile:hasRole rdf:resource="http://www.w3.org/ns/dx/prof/role/guidance"/>
    <dct:conformsTo rdf:resource="https://www.w3.org/TR/html/"/>
    <rdf:type rdf:resource="http://www.w3.org/ns/dx/prof/ResourceDescriptor"/>
    <dct:title>Guides for Data Privacy Vocabulary</dct:title>
  </rdf:Description>
  <rdf:Description rdf:nodeID="person-julian-flake">
    <rdf:type rdf:resource="http://xmlns.com/foaf/0.1/Person"/>
    <rdf:type rdf:resource="http://purl.org/dc/terms/Agent"/>
    <org:memberOf rdf:nodeID="org-university-of-koblenz"/>
    <scoro:hasORCID>0009-0006-4623-1463</scoro:hasORCID>
    <foaf:name>Julian Flake</foaf:name>
  </rdf:Description>
  <rdf:Description rdf:about="https://w3id.org/dpv/primer">
    <rdf:type rdf:resource="http://www.w3.org/ns/dx/prof/ResourceDescriptor"/>
    <profile:hasRole rdf:resource="http://www.w3.org/ns/dx/prof/role/guidance"/>
    <dct:format rdf:resource="https://www.iana.org/assignments/media-types/text/html"/>
    <dct:conformsTo rdf:resource="https://www.w3.org/TR/html/"/>
    <profile:hasArtifact rdf:resource="https://w3id.org/dpv/primer"/>
    <dct:title>Primer for Data Privacy Vocabulary</dct:title>
  </rdf:Description>
  <rdf:Description rdf:about="https://w3id.org/dpv/sector/health/owl#serialisation-html">
    <profile:hasRole rdf:resource="http://www.w3.org/ns/dx/prof/role/specification"/>
    <dct:format rdf:resource="https://www.iana.org/assignments/media-types/text/html"/>
    <dct:conformsTo rdf:resource="https://www.w3.org/TR/html/"/>
    <rdf:type rdf:resource="http://www.w3.org/ns/dx/prof/ResourceDescriptor"/>
    <profile:hasArtifact rdf:resource="https://w3id.org/dpv/sector/health/sector-health-owl.html"/>
    <dct:title>Health Sector Concepts - HTML serialisation</dct:title>
  </rdf:Description>
  <rdf:Description rdf:nodeID="org-ai-accountability-lab-aial-trinity-college-dublin">
    <foaf:name>AI Accountability Lab (AIAL), Trinity College Dublin</foaf:name>
    <rdf:type rdf:resource="http://xmlns.com/foaf/0.1/Organization"/>
  </rdf:Description>
</rdf:RDF>
