@prefix bibo: <http://purl.org/ontology/bibo/> .
@prefix dcam: <http://purl.org/dc/dcam/> .
@prefix dct: <http://purl.org/dc/terms/> .
@prefix dex-owl: <https://w3id.org/dpv/examples/owl#> .
@prefix dpv-owl: <https://w3id.org/dpv/owl#> .
@prefix foaf: <http://xmlns.com/foaf/0.1/> .
@prefix org: <http://www.w3.org/ns/org#> .
@prefix owl: <http://www.w3.org/2002/07/owl#> .
@prefix profile: <http://www.w3.org/ns/dx/prof/> .
@prefix rdf: <http://www.w3.org/1999/02/22-rdf-syntax-ns#> .
@prefix rdfs: <http://www.w3.org/2000/01/rdf-schema#> .
@prefix risk-owl: <https://w3id.org/dpv/risk/owl#> .
@prefix role: <http://www.w3.org/ns/dx/prof/role/> .
@prefix schema: <https://schema.org/> .
@prefix scoro: <http://purl.org/spar/scoro/> .
@prefix skos: <http://www.w3.org/2004/02/skos/core#> .
@prefix sw: <http://www.w3.org/2003/06/sw-vocab-status/ns#> .
@prefix vann: <http://purl.org/vocab/vann/> .
@prefix xsd: <http://www.w3.org/2001/XMLSchema#> .

risk-owl:3LikelihoodLevels a rdfs:Class,
        owl:Class,
        dpv-owl:Likelihood ;
    dct:contributor _:Ne22a67b17c7e4a779c30d2864b6a0cee ;
    dct:created "2022-08-18"^^xsd:date ;
    rdfs:isDefinedBy risk-owl: ;
    rdfs:subClassOf dpv-owl:Likelihood ;
    sw:term_status "accepted"@en ;
    skos:definition "Scale with 3 Likelihood Levels from High to Low"@en ;
    skos:prefLabel "3 Likelihood Levels"@en .

risk-owl:3RiskLevels a rdfs:Class,
        owl:Class,
        dpv-owl:RiskLevel ;
    dct:contributor _:Ne22a67b17c7e4a779c30d2864b6a0cee ;
    dct:created "2022-08-18"^^xsd:date ;
    rdfs:isDefinedBy risk-owl: ;
    rdfs:subClassOf dpv-owl:RiskLevel ;
    sw:term_status "accepted"@en ;
    skos:definition "Scale with 3 Risk Levels from High to Low"@en ;
    skos:prefLabel "3 Risk Levels"@en .

risk-owl:3SeverityLevels a rdfs:Class,
        owl:Class,
        dpv-owl:Severity ;
    dct:contributor _:Ne22a67b17c7e4a779c30d2864b6a0cee ;
    dct:created "2022-08-18"^^xsd:date ;
    rdfs:isDefinedBy risk-owl: ;
    rdfs:subClassOf dpv-owl:Severity ;
    sw:term_status "accepted"@en ;
    skos:definition "Scale with 3 Severity Levels from High to Low"@en ;
    skos:prefLabel "3 Severity Levels"@en .

risk-owl:5LikelihoodLevels a rdfs:Class,
        owl:Class,
        dpv-owl:Likelihood ;
    dct:contributor _:Ne22a67b17c7e4a779c30d2864b6a0cee ;
    dct:created "2022-08-18"^^xsd:date ;
    rdfs:isDefinedBy risk-owl: ;
    rdfs:subClassOf dpv-owl:Likelihood ;
    sw:term_status "accepted"@en ;
    skos:definition "Scale with 5 Likelihood Levels from Very High to Very Low"@en ;
    skos:prefLabel "5 Likelihood Levels"@en .

risk-owl:5RiskLevels a rdfs:Class,
        owl:Class,
        dpv-owl:RiskLevel ;
    dct:contributor _:Ne22a67b17c7e4a779c30d2864b6a0cee ;
    dct:created "2022-08-18"^^xsd:date ;
    rdfs:isDefinedBy risk-owl: ;
    rdfs:subClassOf dpv-owl:RiskLevel ;
    sw:term_status "accepted"@en ;
    skos:definition "Scale with 5 Risk Levels from Very High to Very Low"@en ;
    skos:prefLabel "5 Risk Levels"@en .

risk-owl:5SeverityLevels a rdfs:Class,
        owl:Class,
        dpv-owl:Severity ;
    dct:contributor _:Ne22a67b17c7e4a779c30d2864b6a0cee ;
    dct:created "2022-08-18"^^xsd:date ;
    rdfs:isDefinedBy risk-owl: ;
    rdfs:subClassOf dpv-owl:Severity ;
    sw:term_status "accepted"@en ;
    skos:definition "Scale with 5 Severity Levels from Very High to Very Low"@en ;
    skos:prefLabel "5 Severity Levels"@en .

risk-owl:7LikelihoodLevels a rdfs:Class,
        owl:Class,
        dpv-owl:Likelihood ;
    dct:contributor _:Ne22a67b17c7e4a779c30d2864b6a0cee ;
    dct:created "2022-08-18"^^xsd:date ;
    rdfs:isDefinedBy risk-owl: ;
    rdfs:subClassOf dpv-owl:Likelihood ;
    sw:term_status "accepted"@en ;
    skos:definition "Scale with 7 Likelihood Levels from Extremely High to Extremely Low"@en ;
    skos:prefLabel "7 Likelihood Levels"@en .

risk-owl:7RiskLevels a rdfs:Class,
        owl:Class,
        dpv-owl:RiskLevel ;
    dct:contributor _:Ne22a67b17c7e4a779c30d2864b6a0cee ;
    dct:created "2022-08-18"^^xsd:date ;
    rdfs:isDefinedBy risk-owl: ;
    rdfs:subClassOf dpv-owl:RiskLevel ;
    sw:term_status "accepted"@en ;
    skos:definition "Scale with 7 Risk Levels from Extremely High to Extremely Low"@en ;
    skos:prefLabel "7 Risk Levels"@en .

risk-owl:7SeverityLevels a rdfs:Class,
        owl:Class,
        dpv-owl:Severity ;
    dct:contributor _:Ne22a67b17c7e4a779c30d2864b6a0cee ;
    dct:created "2022-08-18"^^xsd:date ;
    rdfs:isDefinedBy risk-owl: ;
    rdfs:subClassOf dpv-owl:Severity ;
    sw:term_status "accepted"@en ;
    skos:definition "Scale with 7 Severity Levels from Extremely High to Extremely Low"@en ;
    skos:prefLabel "7 Severity Levels"@en .

risk-owl:AccidentalIncident a rdfs:Class,
        owl:Class ;
    dct:created "2024-05-19"^^xsd:date ;
    rdfs:isDefinedBy risk-owl: ;
    rdfs:subClassOf risk-owl:Incident ;
    sw:term_status "accepted"@en ;
    skos:definition "Incident caused due to accidental actions arising from human or human-controlled situations"@en ;
    skos:prefLabel "Accidental Incident"@en .

risk-owl:AccidentalMisuse a rdfs:Class,
        owl:Class,
        dpv-owl:RiskConcept,
        risk-owl:PotentialConsequence,
        risk-owl:PotentialRisk,
        risk-owl:PotentialRiskSource ;
    dct:created "2024-12-17"^^xsd:date ;
    rdfs:isDefinedBy risk-owl: ;
    rdfs:subClassOf risk-owl:Misuse ;
    sw:term_status "accepted"@en ;
    skos:definition "Concept representing accidental misuse (of something)"@en ;
    skos:prefLabel "Accidental Misuse"@en .

risk-owl:AccuracyDegraded a rdfs:Class,
        owl:Class,
        dpv-owl:RiskConcept,
        risk-owl:PotentialConsequence,
        risk-owl:PotentialRisk,
        risk-owl:PotentialRiskSource ;
    dct:contributor _:N9c63c24625fe482386a350b4ea27b4f8,
        _:Ne22a67b17c7e4a779c30d2864b6a0cee ;
    dct:created "2024-12-01"^^xsd:date ;
    rdfs:isDefinedBy risk-owl: ;
    rdfs:subClassOf risk-owl:AccuracyRisk,
        risk-owl:QualityDegraded ;
    sw:term_status "accepted"@en ;
    skos:definition "Concepts representing risks and issues where Accuracy is Degraded"@en ;
    skos:prefLabel "Accuracy Degraded"@en .

risk-owl:AccuracyInconsistent a rdfs:Class,
        owl:Class,
        dpv-owl:RiskConcept,
        risk-owl:PotentialConsequence,
        risk-owl:PotentialRisk,
        risk-owl:PotentialRiskSource ;
    dct:contributor _:Ne22a67b17c7e4a779c30d2864b6a0cee ;
    dct:created "2024-12-01"^^xsd:date ;
    rdfs:isDefinedBy risk-owl: ;
    rdfs:subClassOf risk-owl:AccuracyRisk,
        risk-owl:QualityInconsistent ;
    sw:term_status "accepted"@en ;
    skos:definition "Concepts representing risks and issues where Accuracy is Inconsistent"@en ;
    skos:prefLabel "Accuracy Inconsistent"@en .

risk-owl:AccuracyInsufficient a rdfs:Class,
        owl:Class,
        dpv-owl:RiskConcept,
        risk-owl:PotentialConsequence,
        risk-owl:PotentialRisk,
        risk-owl:PotentialRiskSource ;
    dct:contributor _:N9c63c24625fe482386a350b4ea27b4f8,
        _:Ne22a67b17c7e4a779c30d2864b6a0cee ;
    dct:created "2024-12-01"^^xsd:date ;
    rdfs:isDefinedBy risk-owl: ;
    rdfs:subClassOf risk-owl:AccuracyRisk,
        risk-owl:QualityInsufficient ;
    sw:term_status "accepted"@en ;
    skos:definition "Concepts representing risks and issues where Accuracy is Insufficient"@en ;
    skos:prefLabel "Accuracy Insufficient"@en .

risk-owl:AccuracyRisk a rdfs:Class,
        owl:Class,
        dpv-owl:RiskConcept,
        risk-owl:PotentialConsequence,
        risk-owl:PotentialRisk,
        risk-owl:PotentialRiskSource ;
    dct:contributor _:Ne22a67b17c7e4a779c30d2864b6a0cee ;
    dct:created "2024-12-01"^^xsd:date ;
    rdfs:isDefinedBy risk-owl: ;
    rdfs:subClassOf risk-owl:QualityRisk ;
    sw:term_status "accepted"@en ;
    skos:definition "Concepts representing risks and issues where Accuracy is Risk"@en ;
    skos:prefLabel "Accuracy Risk"@en .

risk-owl:AccuracyUnknown a rdfs:Class,
        owl:Class,
        dpv-owl:RiskConcept,
        risk-owl:PotentialConsequence,
        risk-owl:PotentialRisk,
        risk-owl:PotentialRiskSource ;
    dct:contributor _:Ne22a67b17c7e4a779c30d2864b6a0cee ;
    dct:created "2024-12-01"^^xsd:date ;
    rdfs:isDefinedBy risk-owl: ;
    rdfs:subClassOf risk-owl:AccuracyRisk,
        risk-owl:QualityUnknown ;
    sw:term_status "accepted"@en ;
    skos:definition "Concepts representing risks and issues where Accuracy is Unknown"@en ;
    skos:prefLabel "Accuracy Unknown"@en .

risk-owl:AccuracyUnverified a rdfs:Class,
        owl:Class,
        dpv-owl:RiskConcept,
        risk-owl:PotentialConsequence,
        risk-owl:PotentialRisk,
        risk-owl:PotentialRiskSource ;
    dct:contributor _:Ne22a67b17c7e4a779c30d2864b6a0cee ;
    dct:created "2024-12-01"^^xsd:date ;
    rdfs:isDefinedBy risk-owl: ;
    rdfs:subClassOf risk-owl:AccuracyRisk,
        risk-owl:QualityUnverified ;
    sw:term_status "accepted"@en ;
    skos:definition "Concepts representing risks and issues where Accuracy is Unverified"@en ;
    skos:prefLabel "Accuracy Unverified"@en .

risk-owl:AgeDiscrimination a rdfs:Class,
        owl:Class,
        dpv-owl:RiskConcept,
        risk-owl:PotentialConsequence,
        risk-owl:PotentialImpact,
        risk-owl:PotentialRisk ;
    dct:created "2024-09-30"^^xsd:date ;
    rdfs:isDefinedBy risk-owl: ;
    rdfs:subClassOf risk-owl:Discrimination ;
    sw:term_status "accepted"@en ;
    skos:definition "Discrimination based on a person's age, often impacting older or younger individuals"@en ;
    skos:prefLabel "Age Discrimination"@en .

risk-owl:AuthorisationFailure a rdfs:Class,
        owl:Class,
        dpv-owl:RiskConcept,
        risk-owl:ConfidentialityConcept,
        risk-owl:IntegrityConcept,
        risk-owl:PotentialRisk,
        risk-owl:PotentialRiskSource ;
    dct:contributor _:Ne22a67b17c7e4a779c30d2864b6a0cee ;
    dct:created "2022-08-17"^^xsd:date ;
    dct:modified "2024-08-16"^^xsd:date ;
    dct:source [ a schema:WebPage ;
            schema:name "ENISa Trust Services Security Incidents 2021" ;
            schema:url "https://www.enisa.europa.eu/publications/trust-services-security-incidents-2021" ] ;
    rdfs:isDefinedBy risk-owl: ;
    rdfs:subClassOf risk-owl:OperationalSecurityRisk ;
    sw:term_status "accepted"@en ;
    skos:definition "Concept representing Authorisation Failure"@en ;
    skos:prefLabel "Authorisation Failure"@en .

risk-owl:AvailabilityBreach a rdfs:Class,
        owl:Class,
        dpv-owl:RiskConcept,
        risk-owl:AvailabilityConcept,
        risk-owl:PotentialConsequence,
        risk-owl:PotentialRisk,
        risk-owl:PotentialRiskSource ;
    dct:created "2024-12-17"^^xsd:date ;
    rdfs:isDefinedBy risk-owl: ;
    rdfs:subClassOf risk-owl:DataBreach ;
    sw:term_status "accepted"@en ;
    skos:definition "Concept representing a breach of availability"@en ;
    skos:prefLabel "Availability Breach"@en .

risk-owl:AvailabilityConcept a rdfs:Class,
        owl:Class ;
    dct:contributor _:Ne22a67b17c7e4a779c30d2864b6a0cee ;
    dct:created "2024-09-29"^^xsd:date ;
    rdfs:isDefinedBy risk-owl: ;
    rdfs:subClassOf dpv-owl:RiskConcept ;
    sw:term_status "accepted"@en ;
    skos:definition "Indicates a concept is relevant to 'Availability' in CIA InfoSec model"@en ;
    skos:prefLabel "Availability Concept"@en ;
    skos:scopeNote "This concept allows indicating the applicability of Impact dimension to concepts whether they are a risk source, risk, consequence, or impact"@en .

risk-owl:AvailabilityIncident a rdfs:Class,
        owl:Class ;
    dct:created "2024-05-19"^^xsd:date ;
    rdfs:isDefinedBy risk-owl: ;
    rdfs:subClassOf risk-owl:Incident ;
    sw:term_status "accepted"@en ;
    skos:definition "Incident where the availability of information or system has been affected"@en ;
    skos:prefLabel "Availability Incident"@en .

risk-owl:AvoidConsequence a rdfs:Class,
        owl:Class,
        risk-owl:RiskControl ;
    dct:contributor _:Ne22a67b17c7e4a779c30d2864b6a0cee ;
    dct:created "2025-01-06"^^xsd:date ;
    rdfs:isDefinedBy risk-owl: ;
    rdfs:subClassOf risk-owl:AvoidanceControl,
        risk-owl:ConsequenceControl ;
    sw:term_status "accepted"@en ;
    skos:definition "Control that proactively avoids the consequence such that it has a reduced exposure or applicability in the context"@en ;
    skos:prefLabel "Avoid Consequence"@en .

risk-owl:AvoidImpact a rdfs:Class,
        owl:Class,
        risk-owl:RiskControl ;
    dct:contributor _:Ne22a67b17c7e4a779c30d2864b6a0cee ;
    dct:created "2025-01-06"^^xsd:date ;
    rdfs:isDefinedBy risk-owl: ;
    rdfs:subClassOf risk-owl:AvoidanceControl,
        risk-owl:ImpactControl ;
    sw:term_status "accepted"@en ;
    skos:definition "Control that proactively avoids the impact such that it has a reduced exposure or applicability in the context"@en ;
    skos:prefLabel "Avoid Impact"@en .

risk-owl:AvoidSource a rdfs:Class,
        owl:Class,
        risk-owl:RiskControl ;
    dct:contributor _:Ne22a67b17c7e4a779c30d2864b6a0cee ;
    dct:created "2024-05-19"^^xsd:date ;
    dct:modified "2025-01-06"^^xsd:date ;
    rdfs:isDefinedBy risk-owl: ;
    rdfs:subClassOf risk-owl:AvoidanceControl,
        risk-owl:SourceControl ;
    sw:term_status "modified"@en ;
    skos:definition "Control that proactively avoids the risk source such that it has a reduced exposure or applicability in the context"@en ;
    skos:prefLabel "Avoid Source"@en .

risk-owl:AvoidanceControl a rdfs:Class,
        owl:Class,
        risk-owl:RiskControl ;
    dct:contributor _:Ne22a67b17c7e4a779c30d2864b6a0cee ;
    dct:created "2025-01-06"^^xsd:date ;
    rdfs:isDefinedBy risk-owl: ;
    rdfs:subClassOf risk-owl:ProactiveControl ;
    sw:term_status "accepted"@en ;
    skos:definition "Control that avoids an event with the goal of removing it completely"@en ;
    skos:prefLabel "Avoidance Control"@en ;
    skos:scopeNote "Avoiding is distinct from Mitigation and Modification as the goal to avoid an event is to prevent it from occuring at all, whereas mitigation and modification accept an event will occur and focus on managing it"@en .

risk-owl:BehaviourDistortion a rdfs:Class,
        owl:Class,
        dpv-owl:RiskConcept,
        risk-owl:PotentialConsequence,
        risk-owl:PotentialImpact,
        risk-owl:PotentialRisk ;
    dct:contributor _:N9c63c24625fe482386a350b4ea27b4f8 ;
    dct:created "2024-12-01"^^xsd:date ;
    rdfs:isDefinedBy risk-owl: ;
    rdfs:subClassOf risk-owl:IndividualRisk ;
    sw:term_status "accepted"@en ;
    skos:definition "Concept representing distortion of behaviour of individual(s)"@en ;
    skos:prefLabel "Behaviour Distortion"@en .

risk-owl:BelievesDiscrimination a rdfs:Class,
        owl:Class,
        dpv-owl:RiskConcept,
        risk-owl:PotentialConsequence,
        risk-owl:PotentialImpact,
        risk-owl:PotentialRisk ;
    dct:created "2024-09-30"^^xsd:date ;
    rdfs:isDefinedBy risk-owl: ;
    rdfs:subClassOf risk-owl:Discrimination ;
    sw:term_status "accepted"@en ;
    skos:definition "Discrimination based on a person's beliefs or practices"@en ;
    skos:prefLabel "Believes Discrimination"@en .

risk-owl:Benefit a rdfs:Class,
        owl:Class,
        dpv-owl:RiskConcept,
        risk-owl:PotentialConsequence,
        risk-owl:PotentialImpact,
        risk-owl:PotentialRisk ;
    dct:contributor _:N4b493e90e86f4bec907dc903aaa37183,
        _:N75641c194b3f4973ab2abfb33aed55d3,
        _:N7d9b5ee7f31f4f2ba5951e30b49ec7c0,
        _:Ne22a67b17c7e4a779c30d2864b6a0cee,
        _:Ne58e82a7606b4ab9ada0b0f2f7592231,
        _:Ne84980f7db76425ca367742d2085d8c9 ;
    dct:created "2022-03-23"^^xsd:date ;
    dct:modified "2024-08-16"^^xsd:date ;
    rdfs:isDefinedBy risk-owl: ;
    rdfs:subClassOf risk-owl:Compensation ;
    sw:term_status "accepted"@en ;
    skos:definition "Concept representing benefits - both material and immaterial"@en ;
    skos:prefLabel "Benefit"@en ;
    skos:scopeNote "Even though benefits is filed under organisational concepts, it can be applied to individuals (humans) and groups which are societal"@en .

risk-owl:Bias a rdfs:Class,
        owl:Class,
        dpv-owl:RiskConcept,
        risk-owl:PotentialConsequence,
        risk-owl:PotentialRisk,
        risk-owl:PotentialRiskSource ;
    dct:contributor _:N2e9307242cb14d528effb994db501842,
        _:N9c63c24625fe482386a350b4ea27b4f8,
        _:Ne22a67b17c7e4a779c30d2864b6a0cee ;
    dct:created "2024-09-13"^^xsd:date ;
    dct:source "ISO/IEC 24027:2021"@en ;
    rdfs:isDefinedBy risk-owl: ;
    rdfs:subClassOf risk-owl:TechnicalRiskConcept ;
    sw:term_status "accepted"@en ;
    skos:definition "Bias is defined as the systematic difference in treatment of certain objects, people, or groups in comparison to others"@en ;
    skos:prefLabel "Bias"@en .

risk-owl:Blackmail a rdfs:Class,
        owl:Class,
        dpv-owl:RiskConcept,
        risk-owl:ConfidentialityConcept,
        risk-owl:PotentialConsequence,
        risk-owl:PotentialRisk,
        risk-owl:PotentialRiskSource ;
    dct:contributor _:Ne22a67b17c7e4a779c30d2864b6a0cee ;
    dct:created "2022-08-17"^^xsd:date ;
    dct:modified "2024-08-16"^^xsd:date ;
    dct:source [ a schema:WebPage ;
            schema:name "ISO/IEC 27005:2018" ;
            schema:url "https://www.iso.org/standard/75281.html" ] ;
    rdfs:isDefinedBy risk-owl: ;
    rdfs:subClassOf risk-owl:MaliciousActivity ;
    sw:term_status "accepted"@en ;
    skos:definition "Concept representing Blackmail"@en ;
    skos:prefLabel "Blackmail"@en .

risk-owl:BruteForceAuthorisations a rdfs:Class,
        owl:Class,
        dpv-owl:RiskConcept,
        risk-owl:ConfidentialityConcept,
        risk-owl:IntegrityConcept,
        risk-owl:PotentialRisk,
        risk-owl:PotentialRiskSource ;
    dct:contributor _:Ne22a67b17c7e4a779c30d2864b6a0cee ;
    dct:created "2022-08-17"^^xsd:date ;
    dct:modified "2024-08-16"^^xsd:date ;
    dct:source [ a schema:WebPage ;
            schema:name "ENISA Reference Incident Classification Taxonomy 2018" ;
            schema:url "https://www.enisa.europa.eu/publications/reference-incident-classification-taxonomy/" ] ;
    rdfs:isDefinedBy risk-owl: ;
    rdfs:subClassOf risk-owl:SecurityAttack ;
    sw:term_status "accepted"@en ;
    skos:definition "Concept representing Brute Force Authorisations i.e. bypassing authorisations through brute forcing techniques"@en ;
    skos:prefLabel "Brute Force Authorisations"@en .

risk-owl:CasteDiscrimination a rdfs:Class,
        owl:Class,
        dpv-owl:RiskConcept,
        risk-owl:PotentialConsequence,
        risk-owl:PotentialImpact,
        risk-owl:PotentialRisk ;
    dct:created "2024-09-30"^^xsd:date ;
    rdfs:isDefinedBy risk-owl: ;
    rdfs:subClassOf risk-owl:Discrimination ;
    sw:term_status "accepted"@en ;
    skos:definition "Discrimination based on a person's caste, a form of social stratification found in some cultures"@en ;
    skos:prefLabel "Caste Discrimination"@en .

risk-owl:ChangeConsequence a rdfs:Class,
        owl:Class,
        risk-owl:RiskControl ;
    dct:contributor _:Ne22a67b17c7e4a779c30d2864b6a0cee ;
    dct:created "2024-05-19"^^xsd:date ;
    dct:modified "2025-01-06"^^xsd:date ;
    rdfs:isDefinedBy risk-owl: ;
    rdfs:subClassOf risk-owl:ConsequenceControl,
        risk-owl:SubstitutionControl ;
    sw:term_status "modified"@en ;
    skos:definition "Control that proactively changes the consequence event such that one event is replaced with the occurence or applicability of another event in the context"@en ;
    skos:prefLabel "Change Consequence"@en .

risk-owl:ChangeImpact a rdfs:Class,
        owl:Class,
        risk-owl:RiskControl ;
    dct:contributor _:Ne22a67b17c7e4a779c30d2864b6a0cee ;
    dct:created "2024-05-19"^^xsd:date ;
    dct:modified "2025-01-06"^^xsd:date ;
    rdfs:isDefinedBy risk-owl: ;
    rdfs:subClassOf risk-owl:ImpactControl,
        risk-owl:SubstitutionControl ;
    sw:term_status "modified"@en ;
    skos:definition "Control that proactively changes the impact event such that one event is replaced with the occurence or applicability of another event in the context"@en ;
    skos:prefLabel "Change Impact"@en .

risk-owl:Coercion a rdfs:Class,
        owl:Class,
        dpv-owl:RiskConcept,
        risk-owl:ConfidentialityConcept,
        risk-owl:PotentialConsequence,
        risk-owl:PotentialRisk,
        risk-owl:PotentialRiskSource ;
    dct:contributor _:Ne22a67b17c7e4a779c30d2864b6a0cee ;
    dct:created "2022-08-17"^^xsd:date ;
    dct:modified "2024-08-16"^^xsd:date ;
    dct:source [ a schema:WebPage ;
            schema:name "ENISA Threat Taxonomy 2016" ;
            schema:url "https://www.enisa.europa.eu/topics/threat-risk-management/threats-and-trends/enisa-threat-landscape/threat-taxonomy/view" ] ;
    rdfs:isDefinedBy risk-owl: ;
    rdfs:subClassOf risk-owl:MaliciousActivity ;
    sw:term_status "accepted"@en ;
    skos:definition "Concept representing Coercion"@en ;
    skos:prefLabel "Coercion"@en .

risk-owl:CognitiveBias a rdfs:Class,
        owl:Class,
        dpv-owl:RiskConcept,
        risk-owl:PotentialConsequence,
        risk-owl:PotentialRisk,
        risk-owl:PotentialRiskSource ;
    dct:contributor _:N2e9307242cb14d528effb994db501842,
        _:N9c63c24625fe482386a350b4ea27b4f8,
        _:Ne22a67b17c7e4a779c30d2864b6a0cee ;
    dct:created "2024-09-13"^^xsd:date ;
    dct:source "ISO/IEC 24027:2021"@en ;
    rdfs:isDefinedBy risk-owl: ;
    rdfs:subClassOf risk-owl:Bias ;
    sw:term_status "accepted"@en ;
    skos:definition "Bias that occurs when humans are processing and interpreting information"@en ;
    skos:prefLabel "Cognitive Bias"@en .

risk-owl:Compensation a rdfs:Class,
        owl:Class,
        dpv-owl:RiskConcept,
        risk-owl:PotentialConsequence,
        risk-owl:PotentialImpact,
        risk-owl:PotentialRisk ;
    dct:contributor _:N7d9b5ee7f31f4f2ba5951e30b49ec7c0,
        _:Ne22a67b17c7e4a779c30d2864b6a0cee ;
    dct:created "2024-04-14"^^xsd:date ;
    dct:modified "2024-08-16"^^xsd:date ;
    rdfs:isDefinedBy risk-owl: ;
    rdfs:subClassOf risk-owl:Renumeration ;
    sw:term_status "accepted"@en ;
    skos:definition "Something that acts as or provides compensation - which can be monetary and financial or in other forms"@en ;
    skos:prefLabel "Compensation"@en .

risk-owl:ComponentFailure a rdfs:Class,
        owl:Class,
        dpv-owl:RiskConcept,
        risk-owl:AvailabilityConcept,
        risk-owl:PotentialConsequence,
        risk-owl:PotentialRisk,
        risk-owl:PotentialRiskSource ;
    dct:contributor _:N9c63c24625fe482386a350b4ea27b4f8 ;
    dct:created "2024-12-01"^^xsd:date ;
    rdfs:isDefinedBy risk-owl: ;
    rdfs:subClassOf risk-owl:OperationalSecurityRisk ;
    sw:term_status "accepted"@en ;
    skos:definition "Concept representing Component Failure"@en ;
    skos:prefLabel "Component Failure"@en ;
    skos:scopeNote "Here component refers to both physical and virtual components. The failure of a component may or may not also cause a failure in other related components or the systems they are part of"@en .

risk-owl:ComponentMalfunction a rdfs:Class,
        owl:Class,
        dpv-owl:RiskConcept,
        risk-owl:AvailabilityConcept,
        risk-owl:PotentialConsequence,
        risk-owl:PotentialRisk,
        risk-owl:PotentialRiskSource ;
    dct:contributor _:N9c63c24625fe482386a350b4ea27b4f8 ;
    dct:created "2024-12-01"^^xsd:date ;
    rdfs:isDefinedBy risk-owl: ;
    rdfs:subClassOf risk-owl:OperationalSecurityRisk ;
    sw:term_status "accepted"@en ;
    skos:definition "Concept representing Component Malfunction"@en ;
    skos:prefLabel "Component Malfunction"@en ;
    skos:scopeNote "Here component refers to both physical and virtual components. The malfunction of a component may or may not also cause a malfunction in other related components or the systems they are part of"@en .

risk-owl:CompromiseAccount a rdfs:Class,
        owl:Class,
        dpv-owl:RiskConcept,
        risk-owl:AvailabilityConcept,
        risk-owl:ConfidentialityConcept,
        risk-owl:IntegrityConcept,
        risk-owl:PotentialConsequence,
        risk-owl:PotentialRisk,
        risk-owl:PotentialRiskSource ;
    dct:contributor _:Ne22a67b17c7e4a779c30d2864b6a0cee ;
    dct:created "2022-08-17"^^xsd:date ;
    dct:modified "2024-08-16"^^xsd:date ;
    dct:source [ a schema:WebPage ;
            schema:name "ENISA Reference Incident Classification Taxonomy 2018" ;
            schema:url "https://www.enisa.europa.eu/publications/reference-incident-classification-taxonomy/" ] ;
    rdfs:isDefinedBy risk-owl: ;
    rdfs:subClassOf risk-owl:ExternalSecurityThreat ;
    sw:term_status "accepted"@en ;
    skos:definition "Concept representing a compromised account that is then used by the compromiser"@en ;
    skos:prefLabel "Compromise Account"@en .

risk-owl:CompromiseAccountCredentials a rdfs:Class,
        owl:Class,
        dpv-owl:RiskConcept,
        risk-owl:ConfidentialityConcept,
        risk-owl:PotentialConsequence,
        risk-owl:PotentialRisk,
        risk-owl:PotentialRiskSource ;
    dct:contributor _:Ne22a67b17c7e4a779c30d2864b6a0cee ;
    dct:created "2022-08-17"^^xsd:date ;
    dct:modified "2024-08-16"^^xsd:date ;
    dct:source [ a schema:WebPage ;
            schema:name "ENISA Reference Incident Classification Taxonomy 2018" ;
            schema:url "https://www.enisa.europa.eu/publications/reference-incident-classification-taxonomy/" ] ;
    rdfs:isDefinedBy risk-owl: ;
    rdfs:subClassOf risk-owl:ExternalSecurityThreat ;
    sw:term_status "accepted"@en ;
    skos:definition "Concept representing Account Credentials to be compromised"@en ;
    skos:prefLabel "Compromise Account Credentials"@en .

risk-owl:ConfidentialityBreach a rdfs:Class,
        owl:Class,
        dpv-owl:RiskConcept,
        risk-owl:ConfidentialityConcept,
        risk-owl:PotentialConsequence,
        risk-owl:PotentialRisk,
        risk-owl:PotentialRiskSource ;
    dct:contributor _:Ne22a67b17c7e4a779c30d2864b6a0cee ;
    dct:created "2022-08-17"^^xsd:date ;
    dct:modified "2024-08-16"^^xsd:date ;
    dct:source [ a schema:WebPage ;
            schema:name "ISO/IEC 27005:2018" ;
            schema:url "https://www.iso.org/standard/75281.html" ] ;
    rdfs:isDefinedBy risk-owl: ;
    rdfs:subClassOf risk-owl:DataBreach ;
    sw:term_status "accepted"@en ;
    skos:definition "Concept representing a breach of confidentiality"@en ;
    skos:prefLabel "Confidentiality Breach"@en .

risk-owl:ConfidentialityConcept a rdfs:Class,
        owl:Class ;
    dct:contributor _:Ne22a67b17c7e4a779c30d2864b6a0cee ;
    dct:created "2024-09-29"^^xsd:date ;
    rdfs:isDefinedBy risk-owl: ;
    rdfs:subClassOf dpv-owl:RiskConcept ;
    sw:term_status "accepted"@en ;
    skos:definition "Indicates a concept is relevant to 'Confidentiality' in CIA InfoSec model"@en ;
    skos:prefLabel "Confidentiality Concept"@en ;
    skos:scopeNote "This concept allows indicating the applicability of Confidentiality dimension to concepts whether they are a risk source, risk, consequence, or impact"@en .

risk-owl:ConfidentialityIncident a rdfs:Class,
        owl:Class ;
    dct:created "2024-05-19"^^xsd:date ;
    rdfs:isDefinedBy risk-owl: ;
    rdfs:subClassOf risk-owl:Incident ;
    sw:term_status "accepted"@en ;
    skos:definition "Incident where the confidentiality of information or system has been affected"@en ;
    skos:prefLabel "Confidentiality Incident"@en .

risk-owl:ConfirmationBias a rdfs:Class,
        owl:Class,
        dpv-owl:RiskConcept,
        risk-owl:PotentialConsequence,
        risk-owl:PotentialRisk,
        risk-owl:PotentialRiskSource ;
    dct:contributor _:N2e9307242cb14d528effb994db501842,
        _:N9c63c24625fe482386a350b4ea27b4f8,
        _:Ne22a67b17c7e4a779c30d2864b6a0cee ;
    dct:created "2024-09-13"^^xsd:date ;
    dct:source "ISO/IEC 24027:2021"@en ;
    rdfs:isDefinedBy risk-owl: ;
    rdfs:subClassOf risk-owl:CognitiveBias ;
    sw:term_status "accepted"@en ;
    skos:definition "Bias that occurs when hypotheses, regardless of their veracity, are more likely to be confirmed by the intentional or unintentional interpretation of information"@en ;
    skos:prefLabel "Confirmation Bias"@en .

risk-owl:ConfoundingVariablesBias a rdfs:Class,
        owl:Class,
        dpv-owl:RiskConcept,
        risk-owl:PotentialConsequence,
        risk-owl:PotentialRisk,
        risk-owl:PotentialRiskSource ;
    dct:contributor _:N2e9307242cb14d528effb994db501842,
        _:N9c63c24625fe482386a350b4ea27b4f8,
        _:Ne22a67b17c7e4a779c30d2864b6a0cee ;
    dct:created "2024-09-13"^^xsd:date ;
    dct:source "ISO/IEC 24027:2021"@en ;
    rdfs:isDefinedBy risk-owl: ;
    rdfs:subClassOf risk-owl:StatisticalBias ;
    sw:term_status "accepted"@en ;
    skos:definition "Bias that occurs as a confounding variable that influences both the dependent variable and independent variable causing a spurious association"@en ;
    skos:prefLabel "Confounding Variables Bias"@en .

risk-owl:ConsequenceControl a rdfs:Class,
        owl:Class,
        risk-owl:RiskControl ;
    dct:contributor _:Ne22a67b17c7e4a779c30d2864b6a0cee ;
    dct:created "2024-05-19"^^xsd:date ;
    dct:modified "2025-01-06"^^xsd:date ;
    rdfs:isDefinedBy risk-owl: ;
    rdfs:subClassOf risk-owl:RiskControl ;
    sw:term_status "modified"@en ;
    skos:definition "Risk control for managing consequences"@en ;
    skos:prefLabel "Consequence Control"@en .

risk-owl:ContainmentControl a rdfs:Class,
        owl:Class,
        risk-owl:RiskControl ;
    dct:contributor _:N9c63c24625fe482386a350b4ea27b4f8,
        _:Ne22a67b17c7e4a779c30d2864b6a0cee ;
    dct:created "2024-05-19"^^xsd:date ;
    dct:modified "2025-01-06"^^xsd:date ;
    rdfs:isDefinedBy risk-owl: ;
    rdfs:subClassOf risk-owl:ReductionControl ;
    sw:term_status "modified"@en ;
    skos:definition "Control that aims to contain the event in terms of limiting its occurence or effects"@en ;
    skos:prefLabel "Containment Control"@en ;
    skos:scopeNote "Containment implies either changing the event or the context such that the event's effects are restricted, such as by establishing a physical or digital boundary within which the effects can occur or to prevent the effects from affecting things inside the boundary"@en .

risk-owl:CopyrightViolation a rdfs:Class,
        owl:Class,
        dpv-owl:RiskConcept,
        risk-owl:PotentialConsequence,
        risk-owl:PotentialRisk ;
    dct:contributor _:Ne22a67b17c7e4a779c30d2864b6a0cee ;
    dct:created "2022-08-17"^^xsd:date ;
    dct:modified "2024-08-16"^^xsd:date ;
    dct:source [ a schema:WebPage ;
            schema:name "ENISA Reference Incident Classification Taxonomy 2018" ;
            schema:url "https://www.enisa.europa.eu/publications/reference-incident-classification-taxonomy/" ] ;
    rdfs:isDefinedBy risk-owl: ;
    rdfs:subClassOf risk-owl:LegalComplianceRisk,
        risk-owl:ViolatingObligation ;
    sw:term_status "accepted"@en ;
    skos:definition "Concept representing Copyright Violation"@en ;
    skos:prefLabel "Copyright Violation"@en .

risk-owl:CoverageBias a rdfs:Class,
        owl:Class,
        dpv-owl:RiskConcept,
        risk-owl:PotentialConsequence,
        risk-owl:PotentialRisk,
        risk-owl:PotentialRiskSource ;
    dct:contributor _:N2e9307242cb14d528effb994db501842,
        _:N9c63c24625fe482386a350b4ea27b4f8,
        _:Ne22a67b17c7e4a779c30d2864b6a0cee ;
    dct:created "2024-09-13"^^xsd:date ;
    dct:source "ISO/IEC 24027:2021"@en ;
    rdfs:isDefinedBy risk-owl: ;
    rdfs:subClassOf risk-owl:SelectionBias ;
    sw:term_status "accepted"@en ;
    skos:definition "Bias that occurs when a population represented in a dataset does not match the actual or real population that are being used"@en ;
    skos:prefLabel "Coverage Bias"@en .

risk-owl:CrossBorderIncident a rdfs:Class,
        owl:Class ;
    dct:created "2024-05-19"^^xsd:date ;
    rdfs:isDefinedBy risk-owl: ;
    rdfs:subClassOf risk-owl:Incident ;
    sw:term_status "accepted"@en ;
    skos:definition "Incident involving cross-border or multiple jurisdictions"@en ;
    skos:prefLabel "Cross-Border Incident"@en .

risk-owl:Cryptojacking a rdfs:Class,
        owl:Class,
        dpv-owl:RiskConcept,
        risk-owl:AvailabilityConcept,
        risk-owl:PotentialRisk,
        risk-owl:PotentialRiskSource ;
    dct:contributor _:Ne22a67b17c7e4a779c30d2864b6a0cee ;
    dct:created "2022-08-17"^^xsd:date ;
    dct:modified "2024-08-16"^^xsd:date ;
    dct:source [ a schema:WebPage ;
            schema:name "ENISA Threat Landscape 2021" ;
            schema:url "https://www.enisa.europa.eu/publications/enisa-threat-landscape-2021" ] ;
    rdfs:isDefinedBy risk-owl: ;
    rdfs:subClassOf risk-owl:SecurityAttack ;
    sw:term_status "accepted"@en ;
    skos:definition "Concept representing Cryptojacking"@en ;
    skos:prefLabel "Cryptojacking"@en .

risk-owl:CustomerSupportLimited a rdfs:Class,
        owl:Class,
        dpv-owl:RiskConcept,
        risk-owl:PotentialConsequence,
        risk-owl:PotentialImpact,
        risk-owl:PotentialRisk ;
    dct:created "2024-10-21"^^xsd:date ;
    rdfs:isDefinedBy risk-owl: ;
    rdfs:subClassOf risk-owl:ServiceRelatedConsequence ;
    sw:term_status "accepted"@en ;
    skos:definition "Concept representing customer support to be limited"@en ;
    skos:prefLabel "Customer Support Limited"@en .

risk-owl:Damage a rdfs:Class,
        owl:Class,
        dpv-owl:RiskConcept,
        risk-owl:PotentialConsequence,
        risk-owl:PotentialImpact,
        risk-owl:PotentialRisk ;
    dct:contributor _:Ne22a67b17c7e4a779c30d2864b6a0cee ;
    dct:created "2022-03-30"^^xsd:date ;
    dct:modified "2024-08-16"^^xsd:date ;
    rdfs:isDefinedBy risk-owl: ;
    rdfs:subClassOf risk-owl:LegallyRelevantConsequence ;
    sw:term_status "accepted"@en ;
    skos:definition "Concept representing Damage"@en ;
    skos:prefLabel "Damage"@en .

risk-owl:DataAggregationBias a rdfs:Class,
        owl:Class,
        dpv-owl:RiskConcept,
        risk-owl:PotentialConsequence,
        risk-owl:PotentialRisk,
        risk-owl:PotentialRiskSource ;
    dct:contributor _:N2e9307242cb14d528effb994db501842,
        _:N9c63c24625fe482386a350b4ea27b4f8,
        _:Ne22a67b17c7e4a779c30d2864b6a0cee ;
    dct:created "2024-09-13"^^xsd:date ;
    dct:source "ISO/IEC 24027:2021"@en ;
    rdfs:isDefinedBy risk-owl: ;
    rdfs:subClassOf risk-owl:DataBias ;
    sw:term_status "accepted"@en ;
    skos:definition "Bias that occurs when aggregating data covering different groups of objects has different statistical distributions that introduce bias into the data"@en ;
    skos:prefLabel "Data Aggregation Bias"@en .

risk-owl:DataBias a rdfs:Class,
        owl:Class,
        dpv-owl:RiskConcept,
        risk-owl:PotentialConsequence,
        risk-owl:PotentialRisk,
        risk-owl:PotentialRiskSource ;
    dct:contributor _:N2e9307242cb14d528effb994db501842,
        _:N9c63c24625fe482386a350b4ea27b4f8,
        _:Ne22a67b17c7e4a779c30d2864b6a0cee ;
    dct:created "2024-09-13"^^xsd:date ;
    dct:source "ISO/IEC 24027:2021"@en ;
    rdfs:isDefinedBy risk-owl: ;
    rdfs:subClassOf risk-owl:Bias,
        risk-owl:DataRisk ;
    sw:term_status "accepted"@en ;
    skos:definition "Bias that occurs when data properties that if unaddressed lead to systems that perform better or worse for different groups"@en ;
    skos:prefLabel "Data Bias"@en .

risk-owl:DataBreach a rdfs:Class,
        owl:Class,
        dpv-owl:RiskConcept,
        risk-owl:AvailabilityConcept,
        risk-owl:ConfidentialityConcept,
        risk-owl:IntegrityConcept,
        risk-owl:PotentialConsequence,
        risk-owl:PotentialRisk,
        risk-owl:PotentialRiskSource ;
    dct:contributor _:Ne22a67b17c7e4a779c30d2864b6a0cee ;
    dct:created "2022-08-17"^^xsd:date ;
    dct:modified "2024-08-16"^^xsd:date ;
    dct:source [ a schema:WebPage ;
            schema:name "ISO/IEC 27005:2018" ;
            schema:url "https://www.iso.org/standard/75281.html" ] ;
    vann:example dex-owl:E0069,
        dex-owl:E0071 ;
    rdfs:isDefinedBy risk-owl: ;
    rdfs:subClassOf risk-owl:SecurityBreach ;
    sw:term_status "accepted"@en ;
    skos:definition "Concept representing Data Breach"@en ;
    skos:prefLabel "Data Breach"@en .

risk-owl:DataCollectionError a rdfs:Class,
        owl:Class,
        dpv-owl:RiskConcept,
        risk-owl:PotentialConsequence,
        risk-owl:PotentialRisk,
        risk-owl:PotentialRiskSource ;
    dct:contributor _:N9c63c24625fe482386a350b4ea27b4f8,
        _:Ne22a67b17c7e4a779c30d2864b6a0cee ;
    dct:created "2024-12-01"^^xsd:date ;
    rdfs:isDefinedBy risk-owl: ;
    rdfs:subClassOf risk-owl:DataProcessingError ;
    sw:term_status "accepted"@en ;
    skos:definition "Concept representing error related to data collection"@en ;
    skos:prefLabel "Data Collection Error"@en .

risk-owl:DataCorruption a rdfs:Class,
        owl:Class,
        dpv-owl:RiskConcept,
        risk-owl:IntegrityConcept,
        risk-owl:PotentialConsequence,
        risk-owl:PotentialRisk,
        risk-owl:PotentialRiskSource ;
    dct:contributor _:Ne22a67b17c7e4a779c30d2864b6a0cee ;
    dct:created "2022-08-17"^^xsd:date ;
    dct:modified "2024-08-16"^^xsd:date ;
    dct:source [ a schema:WebPage ;
            schema:name "ISO/IEC 27005:2018" ;
            schema:url "https://www.iso.org/standard/75281.html" ] ;
    rdfs:isDefinedBy risk-owl: ;
    rdfs:subClassOf risk-owl:OperationalSecurityRisk ;
    sw:term_status "modified"@en ;
    skos:definition "Concept representing Corruption of Data"@en ;
    skos:prefLabel "Data Corruption"@en ;
    skos:scopeNote "This concept was called \"Corruption Data\" in DPV 2.0"@en .

risk-owl:DataErasureError a rdfs:Class,
        owl:Class,
        dpv-owl:RiskConcept,
        risk-owl:PotentialConsequence,
        risk-owl:PotentialRisk,
        risk-owl:PotentialRiskSource ;
    dct:contributor _:N9c63c24625fe482386a350b4ea27b4f8,
        _:Ne22a67b17c7e4a779c30d2864b6a0cee ;
    dct:created "2024-12-01"^^xsd:date ;
    rdfs:isDefinedBy risk-owl: ;
    rdfs:subClassOf risk-owl:DataProcessingError ;
    sw:term_status "accepted"@en ;
    skos:definition "Concept representing error related to data erasure"@en ;
    skos:prefLabel "Data Erasure Error"@en .

risk-owl:DataInaccurate a rdfs:Class,
        owl:Class,
        dpv-owl:RiskConcept,
        risk-owl:PotentialConsequence,
        risk-owl:PotentialRisk,
        risk-owl:PotentialRiskSource ;
    dct:contributor _:N9c63c24625fe482386a350b4ea27b4f8,
        _:Ne22a67b17c7e4a779c30d2864b6a0cee ;
    dct:created "2024-12-01"^^xsd:date ;
    rdfs:isDefinedBy risk-owl: ;
    rdfs:subClassOf risk-owl:DataRisk ;
    sw:term_status "accepted"@en ;
    skos:definition "Concept representing data being inaccurate"@en ;
    skos:prefLabel "Data Inaccurate"@en .

risk-owl:DataIncomplete a rdfs:Class,
        owl:Class,
        dpv-owl:RiskConcept,
        risk-owl:PotentialConsequence,
        risk-owl:PotentialRisk,
        risk-owl:PotentialRiskSource ;
    dct:contributor _:N9c63c24625fe482386a350b4ea27b4f8,
        _:Ne22a67b17c7e4a779c30d2864b6a0cee ;
    dct:created "2024-12-01"^^xsd:date ;
    rdfs:isDefinedBy risk-owl: ;
    rdfs:subClassOf risk-owl:DataRisk ;
    sw:term_status "accepted"@en ;
    skos:definition "Concept representing data being incomplete"@en ;
    skos:prefLabel "Data Incomplete"@en .

risk-owl:DataInconsistent a rdfs:Class,
        owl:Class,
        dpv-owl:RiskConcept,
        risk-owl:PotentialConsequence,
        risk-owl:PotentialRisk,
        risk-owl:PotentialRiskSource ;
    dct:contributor _:N9c63c24625fe482386a350b4ea27b4f8,
        _:Ne22a67b17c7e4a779c30d2864b6a0cee ;
    dct:created "2024-12-01"^^xsd:date ;
    rdfs:isDefinedBy risk-owl: ;
    rdfs:subClassOf risk-owl:DataRisk ;
    sw:term_status "accepted"@en ;
    skos:definition "Concept representing data being inconsistent"@en ;
    skos:prefLabel "Data Inconsistent"@en .

risk-owl:DataMisclassified a rdfs:Class,
        owl:Class,
        dpv-owl:RiskConcept,
        risk-owl:PotentialConsequence,
        risk-owl:PotentialRisk,
        risk-owl:PotentialRiskSource ;
    dct:contributor _:N9c63c24625fe482386a350b4ea27b4f8,
        _:Ne22a67b17c7e4a779c30d2864b6a0cee ;
    dct:created "2024-12-01"^^xsd:date ;
    rdfs:isDefinedBy risk-owl: ;
    rdfs:subClassOf risk-owl:DataRisk ;
    sw:term_status "accepted"@en ;
    skos:definition "Concept representing data being misclassified"@en ;
    skos:prefLabel "Data Misclassified"@en .

risk-owl:DataMisinterpretation a rdfs:Class,
        owl:Class,
        dpv-owl:RiskConcept,
        risk-owl:PotentialConsequence,
        risk-owl:PotentialRisk,
        risk-owl:PotentialRiskSource ;
    dct:contributor _:N9c63c24625fe482386a350b4ea27b4f8,
        _:Ne22a67b17c7e4a779c30d2864b6a0cee ;
    dct:created "2024-12-01"^^xsd:date ;
    rdfs:isDefinedBy risk-owl: ;
    rdfs:subClassOf risk-owl:DataRisk ;
    sw:term_status "accepted"@en ;
    skos:definition "Concept representing data being misinterpretation"@en ;
    skos:prefLabel "Data Misinterpretation"@en .

risk-owl:DataNoise a rdfs:Class,
        owl:Class,
        dpv-owl:RiskConcept,
        risk-owl:PotentialConsequence,
        risk-owl:PotentialRisk,
        risk-owl:PotentialRiskSource ;
    dct:contributor _:N9c63c24625fe482386a350b4ea27b4f8,
        _:Ne22a67b17c7e4a779c30d2864b6a0cee ;
    dct:created "2024-12-01"^^xsd:date ;
    rdfs:isDefinedBy risk-owl: ;
    rdfs:subClassOf risk-owl:DataRisk ;
    sw:term_status "accepted"@en ;
    skos:definition "Concept representing data being noise"@en ;
    skos:prefLabel "Data Noise"@en .

risk-owl:DataOutdated a rdfs:Class,
        owl:Class,
        dpv-owl:RiskConcept,
        risk-owl:PotentialConsequence,
        risk-owl:PotentialRisk,
        risk-owl:PotentialRiskSource ;
    dct:contributor _:N9c63c24625fe482386a350b4ea27b4f8,
        _:Ne22a67b17c7e4a779c30d2864b6a0cee ;
    dct:created "2024-12-01"^^xsd:date ;
    rdfs:isDefinedBy risk-owl: ;
    rdfs:subClassOf risk-owl:DataRisk ;
    sw:term_status "accepted"@en ;
    skos:definition "Concept representing data being outdated"@en ;
    skos:prefLabel "Data Outdated"@en .

risk-owl:DataPreparationError a rdfs:Class,
        owl:Class,
        dpv-owl:RiskConcept,
        risk-owl:PotentialConsequence,
        risk-owl:PotentialRisk,
        risk-owl:PotentialRiskSource ;
    dct:contributor _:N9c63c24625fe482386a350b4ea27b4f8,
        _:Ne22a67b17c7e4a779c30d2864b6a0cee ;
    dct:created "2024-12-01"^^xsd:date ;
    rdfs:isDefinedBy risk-owl: ;
    rdfs:subClassOf risk-owl:DataProcessingError ;
    sw:term_status "accepted"@en ;
    skos:definition "Concept representing error related to data preparation"@en ;
    skos:prefLabel "Data Preparation Error"@en .

risk-owl:DataProcessingBias a rdfs:Class,
        owl:Class,
        dpv-owl:RiskConcept,
        risk-owl:PotentialConsequence,
        risk-owl:PotentialRisk,
        risk-owl:PotentialRiskSource ;
    dct:contributor _:N2e9307242cb14d528effb994db501842,
        _:N9c63c24625fe482386a350b4ea27b4f8,
        _:Ne22a67b17c7e4a779c30d2864b6a0cee ;
    dct:created "2024-09-13"^^xsd:date ;
    dct:source "ISO/IEC 24027:2021"@en ;
    rdfs:isDefinedBy risk-owl: ;
    rdfs:subClassOf risk-owl:DataBias ;
    sw:term_status "accepted"@en ;
    skos:definition "Bias that occurs due to pre-processing (or post-processing) of data, even though the original data would not have led to any bias"@en ;
    skos:prefLabel "Data Processing Bias"@en .

risk-owl:DataProcessingError a rdfs:Class,
        owl:Class,
        dpv-owl:RiskConcept,
        risk-owl:PotentialConsequence,
        risk-owl:PotentialRisk,
        risk-owl:PotentialRiskSource ;
    dct:contributor _:N9c63c24625fe482386a350b4ea27b4f8,
        _:Ne22a67b17c7e4a779c30d2864b6a0cee ;
    dct:created "2024-12-01"^^xsd:date ;
    rdfs:isDefinedBy risk-owl: ;
    rdfs:subClassOf risk-owl:DataRisk ;
    sw:term_status "accepted"@en ;
    skos:definition "Concept representing operational error in the processing of data"@en ;
    skos:prefLabel "Data Processing Error"@en .

risk-owl:DataRisk a rdfs:Class,
        owl:Class,
        dpv-owl:RiskConcept,
        risk-owl:PotentialConsequence,
        risk-owl:PotentialRisk,
        risk-owl:PotentialRiskSource ;
    dct:contributor _:N9c63c24625fe482386a350b4ea27b4f8,
        _:Ne22a67b17c7e4a779c30d2864b6a0cee ;
    dct:created "2024-12-01"^^xsd:date ;
    rdfs:isDefinedBy risk-owl: ;
    rdfs:subClassOf risk-owl:TechnicalRiskConcept ;
    sw:term_status "accepted"@en ;
    skos:definition "Risks and risk concepts related to data"@en ;
    skos:prefLabel "Data Risk"@en .

risk-owl:DataSelectionError a rdfs:Class,
        owl:Class,
        dpv-owl:RiskConcept,
        risk-owl:PotentialConsequence,
        risk-owl:PotentialRisk,
        risk-owl:PotentialRiskSource ;
    dct:contributor _:N9c63c24625fe482386a350b4ea27b4f8,
        _:Ne22a67b17c7e4a779c30d2864b6a0cee ;
    dct:created "2024-12-01"^^xsd:date ;
    rdfs:isDefinedBy risk-owl: ;
    rdfs:subClassOf risk-owl:DataProcessingError ;
    sw:term_status "accepted"@en ;
    skos:definition "Concept representing an error in data selection"@en ;
    skos:prefLabel "Data SelectionError"@en .

risk-owl:DataSparse a rdfs:Class,
        owl:Class,
        dpv-owl:RiskConcept,
        risk-owl:PotentialConsequence,
        risk-owl:PotentialRisk,
        risk-owl:PotentialRiskSource ;
    dct:contributor _:N9c63c24625fe482386a350b4ea27b4f8,
        _:Ne22a67b17c7e4a779c30d2864b6a0cee ;
    dct:created "2024-12-01"^^xsd:date ;
    rdfs:isDefinedBy risk-owl: ;
    rdfs:subClassOf risk-owl:DataRisk ;
    sw:term_status "accepted"@en ;
    skos:definition "Concept representing data being sparse"@en ;
    skos:prefLabel "Data Sparse"@en .

risk-owl:DataStorageError a rdfs:Class,
        owl:Class,
        dpv-owl:RiskConcept,
        risk-owl:PotentialConsequence,
        risk-owl:PotentialRisk,
        risk-owl:PotentialRiskSource ;
    dct:contributor _:N9c63c24625fe482386a350b4ea27b4f8,
        _:Ne22a67b17c7e4a779c30d2864b6a0cee ;
    dct:created "2024-12-01"^^xsd:date ;
    rdfs:isDefinedBy risk-owl: ;
    rdfs:subClassOf risk-owl:DataProcessingError ;
    sw:term_status "accepted"@en ;
    skos:definition "Concept representing error related to data storage"@en ;
    skos:prefLabel "Data Storage Error"@en .

risk-owl:DataTransferError a rdfs:Class,
        owl:Class,
        dpv-owl:RiskConcept,
        risk-owl:PotentialConsequence,
        risk-owl:PotentialRisk,
        risk-owl:PotentialRiskSource ;
    dct:contributor _:N9c63c24625fe482386a350b4ea27b4f8,
        _:Ne22a67b17c7e4a779c30d2864b6a0cee ;
    dct:created "2024-12-01"^^xsd:date ;
    rdfs:isDefinedBy risk-owl: ;
    rdfs:subClassOf risk-owl:DataProcessingError ;
    sw:term_status "accepted"@en ;
    skos:definition "Concept representing error related to data transfer"@en ;
    skos:prefLabel "Data Transfer Error"@en .

risk-owl:DataUnavailable a rdfs:Class,
        owl:Class,
        dpv-owl:RiskConcept,
        risk-owl:PotentialConsequence,
        risk-owl:PotentialRisk,
        risk-owl:PotentialRiskSource ;
    dct:contributor _:N9c63c24625fe482386a350b4ea27b4f8,
        _:Ne22a67b17c7e4a779c30d2864b6a0cee ;
    dct:created "2024-12-01"^^xsd:date ;
    rdfs:isDefinedBy risk-owl: ;
    rdfs:subClassOf risk-owl:DataRisk ;
    sw:term_status "accepted"@en ;
    skos:definition "Concept representing data being unavailable"@en ;
    skos:prefLabel "Data Unavailable"@en .

risk-owl:DataUnrepresentative a rdfs:Class,
        owl:Class,
        dpv-owl:RiskConcept,
        risk-owl:PotentialConsequence,
        risk-owl:PotentialRisk,
        risk-owl:PotentialRiskSource ;
    dct:contributor _:N9c63c24625fe482386a350b4ea27b4f8,
        _:Ne22a67b17c7e4a779c30d2864b6a0cee ;
    dct:created "2024-12-01"^^xsd:date ;
    rdfs:isDefinedBy risk-owl: ;
    rdfs:subClassOf risk-owl:DataRisk ;
    sw:term_status "accepted"@en ;
    skos:definition "Concept representing data being unrepresentative"@en ;
    skos:prefLabel "Data Unrepresentative"@en .

risk-owl:DataUnstructured a rdfs:Class,
        owl:Class,
        dpv-owl:RiskConcept,
        risk-owl:PotentialConsequence,
        risk-owl:PotentialRisk,
        risk-owl:PotentialRiskSource ;
    dct:contributor _:N9c63c24625fe482386a350b4ea27b4f8,
        _:Ne22a67b17c7e4a779c30d2864b6a0cee ;
    dct:created "2024-12-01"^^xsd:date ;
    rdfs:isDefinedBy risk-owl: ;
    rdfs:subClassOf risk-owl:DataRisk ;
    sw:term_status "accepted"@en ;
    skos:definition "Concept representing data being unstructured"@en ;
    skos:prefLabel "Data Unstructured"@en .

risk-owl:DataUnverified a rdfs:Class,
        owl:Class,
        dpv-owl:RiskConcept,
        risk-owl:PotentialConsequence,
        risk-owl:PotentialRisk,
        risk-owl:PotentialRiskSource ;
    dct:contributor _:N9c63c24625fe482386a350b4ea27b4f8,
        _:Ne22a67b17c7e4a779c30d2864b6a0cee ;
    dct:created "2024-12-01"^^xsd:date ;
    rdfs:isDefinedBy risk-owl: ;
    rdfs:subClassOf risk-owl:DataRisk ;
    sw:term_status "accepted"@en ;
    skos:definition "Concept representing data being unverified"@en ;
    skos:prefLabel "Data Unverified"@en .

risk-owl:DelayedApplicationProcessing a rdfs:Class,
        owl:Class,
        dpv-owl:RiskConcept,
        risk-owl:PotentialConsequence,
        risk-owl:PotentialImpact,
        risk-owl:PotentialRisk ;
    dct:created "2024-10-21"^^xsd:date ;
    rdfs:isDefinedBy risk-owl: ;
    rdfs:subClassOf risk-owl:ServiceRelatedConsequence ;
    sw:term_status "accepted"@en ;
    skos:definition "Concept representing delayed processing of applications"@en ;
    skos:prefLabel "Delayed Application Processing"@en .

risk-owl:DeliberateIncident a rdfs:Class,
        owl:Class ;
    dct:created "2024-05-19"^^xsd:date ;
    rdfs:isDefinedBy risk-owl: ;
    rdfs:subClassOf risk-owl:Incident ;
    sw:term_status "accepted"@en ;
    skos:definition "Incident caused due to deliberate actions of a human"@en ;
    skos:prefLabel "Deliberate Incident"@en .

risk-owl:DenialServiceAttack a rdfs:Class,
        owl:Class,
        dpv-owl:RiskConcept,
        risk-owl:AvailabilityConcept,
        risk-owl:PotentialRisk,
        risk-owl:PotentialRiskSource ;
    dct:contributor _:Ne22a67b17c7e4a779c30d2864b6a0cee ;
    dct:created "2022-08-17"^^xsd:date ;
    dct:modified "2024-08-16"^^xsd:date ;
    dct:source [ a schema:WebPage ;
            schema:name "ISO/IEC 27005:2018" ;
            schema:url "https://www.iso.org/standard/75281.html" ] ;
    rdfs:isDefinedBy risk-owl: ;
    rdfs:subClassOf risk-owl:SecurityAttack ;
    sw:term_status "accepted"@en ;
    skos:definition "Concept representing Denial of Service Attack (DoS)"@en ;
    skos:prefLabel "Denial of Service Attack (DoS)"@en .

risk-owl:DetectionControl a rdfs:Class,
        owl:Class,
        risk-owl:RiskControl ;
    dct:contributor _:N9c63c24625fe482386a350b4ea27b4f8,
        _:Ne22a67b17c7e4a779c30d2864b6a0cee ;
    dct:created "2024-05-19"^^xsd:date ;
    dct:modified "2025-01-06"^^xsd:date ;
    rdfs:isDefinedBy risk-owl: ;
    rdfs:subClassOf risk-owl:MonitorControl ;
    sw:term_status "modified"@en ;
    skos:definition "Control that detects an event"@en ;
    skos:prefLabel "Detection Control"@en ;
    skos:scopeNote "Detection refers to the observation, derivation, inference, or any other method for drawing conclusions that an event has occurred or is likely to occur with a given certainty. For controls that identify information about the event in terms of metrics or characteristics, see risk:IdentificationControl"@en .

risk-owl:Detriment a rdfs:Class,
        owl:Class,
        dpv-owl:RiskConcept,
        risk-owl:PotentialConsequence,
        risk-owl:PotentialImpact,
        risk-owl:PotentialRisk ;
    dct:contributor _:N4b493e90e86f4bec907dc903aaa37183,
        _:N75641c194b3f4973ab2abfb33aed55d3,
        _:N7d9b5ee7f31f4f2ba5951e30b49ec7c0,
        _:Ne22a67b17c7e4a779c30d2864b6a0cee,
        _:Ne84980f7db76425ca367742d2085d8c9 ;
    dct:created "2022-03-23"^^xsd:date ;
    dct:modified "2024-08-16"^^xsd:date ;
    rdfs:isDefinedBy risk-owl: ;
    rdfs:subClassOf risk-owl:LegallyRelevantConsequence ;
    sw:term_status "accepted"@en ;
    skos:definition "Concept representing Detriment"@en ;
    skos:prefLabel "Detriment"@en .

risk-owl:DirectDiscrimination a rdfs:Class,
        owl:Class,
        dpv-owl:RiskConcept,
        risk-owl:PotentialConsequence,
        risk-owl:PotentialImpact,
        risk-owl:PotentialRisk ;
    dct:created "2024-09-30"^^xsd:date ;
    rdfs:isDefinedBy risk-owl: ;
    rdfs:subClassOf risk-owl:Discrimination ;
    sw:term_status "accepted"@en ;
    skos:definition "Occurs when a person is treated less favorably than another in a comparable situation based on a protected characteristic (e.g., race, sex, disability)"@en ;
    skos:prefLabel "Direct Discrimination"@en .

risk-owl:DisabilityDiscrimination a rdfs:Class,
        owl:Class,
        dpv-owl:RiskConcept,
        risk-owl:PotentialConsequence,
        risk-owl:PotentialImpact,
        risk-owl:PotentialRisk ;
    dct:created "2024-09-30"^^xsd:date ;
    rdfs:isDefinedBy risk-owl: ;
    rdfs:subClassOf risk-owl:Discrimination ;
    sw:term_status "accepted"@en ;
    skos:definition "Discrimination against individuals based on physical or mental disabilities"@en ;
    skos:prefLabel "Disability Discrimination"@en .

risk-owl:Discrimination a rdfs:Class,
        owl:Class,
        dpv-owl:RiskConcept,
        risk-owl:PotentialConsequence,
        risk-owl:PotentialImpact,
        risk-owl:PotentialRisk ;
    dct:contributor _:N7d9b5ee7f31f4f2ba5951e30b49ec7c0 ;
    dct:created "2024-09-30"^^xsd:date ;
    rdfs:isDefinedBy risk-owl: ;
    rdfs:subClassOf risk-owl:SocietalRiskConcept ;
    sw:term_status "accepted"@en ;
    skos:definition "Discrimination is the treatment of a person or particular group of people differently, in a way that is worse than the way people are usually treate"@en ;
    skos:prefLabel "Discrimination"@en .

risk-owl:DisproportionateEnergyConsumption a rdfs:Class,
        owl:Class,
        dpv-owl:RiskConcept,
        risk-owl:PotentialConsequence,
        risk-owl:PotentialImpact,
        risk-owl:PotentialRisk ;
    dct:created "2024-10-21"^^xsd:date ;
    rdfs:isDefinedBy risk-owl: ;
    rdfs:subClassOf risk-owl:EnvironmentalRisk ;
    sw:term_status "accepted"@en ;
    skos:definition "The occurence or potential occurence of disproportionate energy consumption when considering the value obtained from undertaking the activity and the amount of energy being utilised"@en ;
    skos:prefLabel "Disproportionate Energy Consumption"@en .

risk-owl:DistributedDenialServiceAttack a rdfs:Class,
        owl:Class,
        dpv-owl:RiskConcept,
        risk-owl:AvailabilityConcept,
        risk-owl:PotentialRisk,
        risk-owl:PotentialRiskSource ;
    dct:contributor _:Ne22a67b17c7e4a779c30d2864b6a0cee ;
    dct:created "2022-08-17"^^xsd:date ;
    dct:modified "2024-08-16"^^xsd:date ;
    dct:source [ a schema:WebPage ;
            schema:name "ISO/IEC 27005:2018" ;
            schema:url "https://www.iso.org/standard/75281.html" ] ;
    rdfs:isDefinedBy risk-owl: ;
    rdfs:subClassOf risk-owl:DenialServiceAttack ;
    sw:term_status "accepted"@en ;
    skos:definition "Concept representing Distributed Denial of Service Attack (DDoS)"@en ;
    skos:prefLabel "Distributed Denial of Service Attack (DDoS)"@en .

risk-owl:Earthquake a rdfs:Class,
        owl:Class,
        dpv-owl:RiskConcept,
        risk-owl:PotentialConsequence,
        risk-owl:PotentialImpact,
        risk-owl:PotentialRisk ;
    dct:created "2024-10-21"^^xsd:date ;
    rdfs:isDefinedBy risk-owl: ;
    rdfs:subClassOf risk-owl:EnvironmentalRisk ;
    sw:term_status "accepted"@en ;
    skos:definition "The occurence or potential occurence of earthquakes"@en ;
    skos:prefLabel "Earthquake"@en .

risk-owl:EliminationControl a rdfs:Class,
        owl:Class,
        risk-owl:RiskControl ;
    dct:contributor _:N9c63c24625fe482386a350b4ea27b4f8,
        _:Ne22a67b17c7e4a779c30d2864b6a0cee ;
    dct:created "2025-01-06"^^xsd:date ;
    rdfs:isDefinedBy risk-owl: ;
    rdfs:subClassOf risk-owl:AvoidanceControl ;
    sw:term_status "accepted"@en ;
    skos:definition "Control that eliminates an event entirely such that the event does not occur"@en ;
    skos:prefLabel "Elimination Control"@en ;
    skos:scopeNote "Elimination requires the event's likelihood to be reduced to zero such that the event cannot occur in the context. This can be done by establishing methods to prevent the event from occuring (e.g. gatekeeping filters) or by changing the underlying context context (e.g. replacing faulty device). The difference between risk:ModificationControl and risk:EliminationControl is that modification works to change the event characteristics whereas elimination works on the context to prevent the event"@en .

risk-owl:EnvironmentalIncident a rdfs:Class,
        owl:Class ;
    dct:created "2024-05-19"^^xsd:date ;
    rdfs:isDefinedBy risk-owl: ;
    rdfs:subClassOf risk-owl:Incident ;
    sw:term_status "accepted"@en ;
    skos:definition "Incident caused due to environmental factors outside human controls"@en ;
    skos:prefLabel "Environmental Incident"@en .

risk-owl:EnvironmentalRisk a rdfs:Class,
        owl:Class,
        dpv-owl:RiskConcept,
        risk-owl:PotentialConsequence,
        risk-owl:PotentialImpact,
        risk-owl:PotentialRisk ;
    dct:created "2024-10-21"^^xsd:date ;
    rdfs:isDefinedBy risk-owl: ;
    rdfs:subClassOf risk-owl:SocietalRiskConcept ;
    sw:term_status "accepted"@en ;
    skos:definition "Risks and issues that have their origin in environment or can affect the environment at large"@en ;
    skos:prefLabel "Environmental Risk"@en .

risk-owl:EquipmentFailure a rdfs:Class,
        owl:Class,
        dpv-owl:RiskConcept,
        risk-owl:AvailabilityConcept,
        risk-owl:PotentialConsequence,
        risk-owl:PotentialRisk,
        risk-owl:PotentialRiskSource ;
    dct:contributor _:Ne22a67b17c7e4a779c30d2864b6a0cee ;
    dct:created "2022-08-17"^^xsd:date ;
    dct:modified "2024-08-16"^^xsd:date ;
    dct:source [ a schema:WebPage ;
            schema:name "ISO/IEC 27005:2018" ;
            schema:url "https://www.iso.org/standard/75281.html" ] ;
    rdfs:isDefinedBy risk-owl: ;
    rdfs:subClassOf risk-owl:OperationalSecurityRisk ;
    sw:term_status "accepted"@en ;
    skos:definition "Concept representing Equipment Failure"@en ;
    skos:prefLabel "Equipment Failure"@en ;
    skos:scopeNote "Here equipment refers to physical equipment"@en .

risk-owl:EquipmentMalfunction a rdfs:Class,
        owl:Class,
        dpv-owl:RiskConcept,
        risk-owl:AvailabilityConcept,
        risk-owl:PotentialConsequence,
        risk-owl:PotentialRisk,
        risk-owl:PotentialRiskSource ;
    dct:contributor _:Ne22a67b17c7e4a779c30d2864b6a0cee ;
    dct:created "2022-08-17"^^xsd:date ;
    dct:modified "2024-08-16"^^xsd:date ;
    dct:source [ a schema:WebPage ;
            schema:name "ISO/IEC 27005:2018" ;
            schema:url "https://www.iso.org/standard/75281.html" ] ;
    rdfs:isDefinedBy risk-owl: ;
    rdfs:subClassOf risk-owl:OperationalSecurityRisk ;
    sw:term_status "accepted"@en ;
    skos:definition "Concept representing Equipment Malfunction"@en ;
    skos:prefLabel "Equipment Malfunction"@en ;
    skos:scopeNote "Here equipment refers to physical equipment"@en .

risk-owl:ErroneousUse a rdfs:Class,
        owl:Class,
        dpv-owl:RiskConcept,
        risk-owl:PotentialConsequence,
        risk-owl:PotentialRisk,
        risk-owl:PotentialRiskSource ;
    dct:contributor _:Ne22a67b17c7e4a779c30d2864b6a0cee ;
    dct:created "2022-08-17"^^xsd:date ;
    dct:modified "2024-08-16"^^xsd:date ;
    dct:source [ a schema:WebPage ;
            schema:name "ISO/IEC 27005:2018" ;
            schema:url "https://www.iso.org/standard/75281.html" ] ;
    rdfs:isDefinedBy risk-owl: ;
    rdfs:subClassOf risk-owl:UserRisks ;
    sw:term_status "accepted"@en ;
    skos:definition "Concept representing erroneous use (of something)"@en ;
    skos:prefLabel "Erroneous Use"@en .

risk-owl:EthnicDiscrimination a rdfs:Class,
        owl:Class,
        dpv-owl:RiskConcept,
        risk-owl:PotentialConsequence,
        risk-owl:PotentialImpact,
        risk-owl:PotentialRisk ;
    dct:created "2024-09-30"^^xsd:date ;
    rdfs:isDefinedBy risk-owl: ;
    rdfs:subClassOf risk-owl:Racism ;
    sw:term_status "accepted"@en ;
    skos:definition "Discrimination against individuals based on their ethnicity or cultural heritage"@en ;
    skos:prefLabel "Ethnic Discrimination"@en .

risk-owl:ExcellenceDiscrimination a rdfs:Class,
        owl:Class,
        dpv-owl:RiskConcept,
        risk-owl:PotentialConsequence,
        risk-owl:PotentialImpact,
        risk-owl:PotentialRisk ;
    dct:created "2024-09-30"^^xsd:date ;
    rdfs:isDefinedBy risk-owl: ;
    rdfs:subClassOf risk-owl:Discrimination ;
    sw:term_status "accepted"@en ;
    skos:definition "Favoritism towards individuals deemed more competent or superior, often at the expense of others"@en ;
    skos:prefLabel "Excellence Discrimination"@en .

risk-owl:ExposureToHarmfulSpeech a rdfs:Class,
        owl:Class,
        dpv-owl:RiskConcept,
        risk-owl:PotentialConsequence,
        risk-owl:PotentialImpact,
        risk-owl:PotentialRisk ;
    dct:contributor _:Ne22a67b17c7e4a779c30d2864b6a0cee ;
    dct:created "2022-08-17"^^xsd:date ;
    dct:modified "2024-08-16"^^xsd:date ;
    dct:source [ a schema:WebPage ;
            schema:name "ENISA Reference Incident Classification Taxonomy 2018" ;
            schema:url "https://www.enisa.europa.eu/publications/reference-incident-classification-taxonomy/" ] ;
    rdfs:isDefinedBy risk-owl: ;
    rdfs:subClassOf risk-owl:IndividualRisk,
        risk-owl:MentalHealth,
        risk-owl:Wellbeing ;
    sw:term_status "accepted"@en ;
    skos:definition "Concept representing Harmful Speech"@en ;
    skos:prefLabel "Exposure to Harmful Speech"@en ;
    skos:scopeNote "This concept was called \"HarmfulSpeech\" in DPV 2.0"@en .

risk-owl:ExternalSecurityThreat a rdfs:Class,
        owl:Class,
        dpv-owl:RiskConcept,
        risk-owl:PotentialConsequence,
        risk-owl:PotentialRisk,
        risk-owl:PotentialRiskSource ;
    dct:created "2024-12-17"^^xsd:date ;
    rdfs:isDefinedBy risk-owl: ;
    rdfs:subClassOf risk-owl:TechnicalRiskConcept ;
    sw:term_status "accepted"@en ;
    skos:definition "Concepts associated with security threats that are likely to originate externally"@en ;
    skos:prefLabel "External Security Threat"@en .

risk-owl:Extorsion a rdfs:Class,
        owl:Class,
        dpv-owl:RiskConcept,
        risk-owl:ConfidentialityConcept,
        risk-owl:PotentialConsequence,
        risk-owl:PotentialRisk,
        risk-owl:PotentialRiskSource ;
    dct:contributor _:Ne22a67b17c7e4a779c30d2864b6a0cee ;
    dct:created "2022-08-17"^^xsd:date ;
    dct:modified "2024-08-16"^^xsd:date ;
    dct:source [ a schema:WebPage ;
            schema:name "ENISA Threat Taxonomy 2016" ;
            schema:url "https://www.enisa.europa.eu/topics/threat-risk-management/threats-and-trends/enisa-threat-landscape/threat-taxonomy/view" ] ;
    rdfs:isDefinedBy risk-owl: ;
    rdfs:subClassOf risk-owl:MaliciousActivity ;
    sw:term_status "accepted"@en ;
    skos:definition "Concept representing Extorsion"@en ;
    skos:prefLabel "Extorsion"@en .

risk-owl:ExtremelyHighLikelihood a rdfs:Class,
        owl:Class,
        dpv-owl:Likelihood ;
    dct:contributor _:Ne22a67b17c7e4a779c30d2864b6a0cee ;
    dct:created "2022-08-18"^^xsd:date ;
    rdf:value "0.99,xsd:decimal" ;
    rdfs:isDefinedBy risk-owl: ;
    rdfs:subClassOf risk-owl:7LikelihoodLevels ;
    sw:term_status "accepted"@en ;
    skos:definition "Level where Likelihood is Extremely High"@en ;
    skos:prefLabel "Extremely High Likelihood"@en ;
    skos:scopeNote "The suggested quantitative value for this concept is 0.99 on a scale of 0 to 1"@en .

risk-owl:ExtremelyHighRisk a rdfs:Class,
        owl:Class,
        dpv-owl:RiskLevel ;
    dct:contributor _:Ne22a67b17c7e4a779c30d2864b6a0cee ;
    dct:created "2022-08-18"^^xsd:date ;
    rdf:value "0.99,xsd:decimal" ;
    rdfs:isDefinedBy risk-owl: ;
    rdfs:subClassOf risk-owl:7RiskLevels ;
    sw:term_status "accepted"@en ;
    skos:definition "Level where Risk is Extremely High"@en ;
    skos:prefLabel "Extremely High Risk"@en ;
    skos:scopeNote "The suggested quantitative value for this concept is 0.99 on a scale of 0 to 1"@en .

risk-owl:ExtremelyHighSeverity a rdfs:Class,
        owl:Class,
        dpv-owl:Severity ;
    dct:contributor _:Ne22a67b17c7e4a779c30d2864b6a0cee ;
    dct:created "2022-08-18"^^xsd:date ;
    rdf:value "0.99,xsd:decimal" ;
    rdfs:isDefinedBy risk-owl: ;
    rdfs:subClassOf risk-owl:7SeverityLevels ;
    sw:term_status "accepted"@en ;
    skos:definition "Level where Severity is Extremely High"@en ;
    skos:prefLabel "Extremely High Severity"@en ;
    skos:scopeNote "The suggested quantitative value for this concept is 0.99 on a scale of 0 to 1"@en .

risk-owl:ExtremelyLowLikelihood a rdfs:Class,
        owl:Class,
        dpv-owl:Likelihood ;
    dct:contributor _:Ne22a67b17c7e4a779c30d2864b6a0cee ;
    dct:created "2022-08-18"^^xsd:date ;
    rdf:value "0.01,xsd:decimal" ;
    rdfs:isDefinedBy risk-owl: ;
    rdfs:subClassOf risk-owl:7LikelihoodLevels ;
    sw:term_status "accepted"@en ;
    skos:definition "Level where Likelihood is Extremely Low"@en ;
    skos:prefLabel "Extremely Low Likelihood"@en ;
    skos:scopeNote "The suggested quantitative value for this concept is 0.01 on a scale of 0 to 1"@en .

risk-owl:ExtremelyLowRisk a rdfs:Class,
        owl:Class,
        dpv-owl:RiskLevel ;
    dct:contributor _:Ne22a67b17c7e4a779c30d2864b6a0cee ;
    dct:created "2022-08-18"^^xsd:date ;
    rdf:value "0.01,xsd:decimal" ;
    rdfs:isDefinedBy risk-owl: ;
    rdfs:subClassOf risk-owl:7RiskLevels ;
    sw:term_status "accepted"@en ;
    skos:definition "Level where Risk is Extremely Low"@en ;
    skos:prefLabel "Extremely Low Risk"@en ;
    skos:scopeNote "The suggested quantitative value for this concept is 0.01 on a scale of 0 to 1"@en .

risk-owl:ExtremelyLowSeverity a rdfs:Class,
        owl:Class,
        dpv-owl:Severity ;
    dct:contributor _:Ne22a67b17c7e4a779c30d2864b6a0cee ;
    dct:created "2022-08-18"^^xsd:date ;
    rdf:value "0.01,xsd:decimal" ;
    rdfs:isDefinedBy risk-owl: ;
    rdfs:subClassOf risk-owl:7SeverityLevels ;
    sw:term_status "accepted"@en ;
    skos:definition "Level where Severity is Extremely Low"@en ;
    skos:prefLabel "Extremely Low Severity"@en ;
    skos:scopeNote "The suggested quantitative value for this concept is 0.01 on a scale of 0 to 1"@en .

risk-owl:FinancialImpact a rdfs:Class,
        owl:Class,
        dpv-owl:RiskConcept,
        risk-owl:PotentialConsequence,
        risk-owl:PotentialImpact,
        risk-owl:PotentialRisk ;
    dct:created "2024-10-21"^^xsd:date ;
    rdfs:isDefinedBy risk-owl: ;
    rdfs:subClassOf risk-owl:OrganisationalRiskConcept ;
    sw:term_status "accepted"@en ;
    skos:definition "Things that cause or have the potential to impact financial resources"@en ;
    skos:prefLabel "Financial Impact"@en .

risk-owl:FinancialLoss a rdfs:Class,
        owl:Class,
        dpv-owl:RiskConcept,
        risk-owl:PotentialConsequence,
        risk-owl:PotentialImpact,
        risk-owl:PotentialRisk ;
    dct:contributor _:Ne22a67b17c7e4a779c30d2864b6a0cee ;
    dct:created "2022-08-17"^^xsd:date ;
    dct:modified "2024-08-16"^^xsd:date ;
    dct:source [ a schema:WebPage ;
            schema:name "ISO/IEC 27005:2018" ;
            schema:url "https://www.iso.org/standard/75281.html" ] ;
    rdfs:isDefinedBy risk-owl: ;
    rdfs:subClassOf risk-owl:FinancialImpact ;
    sw:term_status "accepted"@en ;
    skos:definition "Concept representing Financial Loss which may be actual loss of existing financial assets or hypothetical loss of financial opportunity"@en ;
    skos:prefLabel "Financial Loss"@en .

risk-owl:Floods a rdfs:Class,
        owl:Class,
        dpv-owl:RiskConcept,
        risk-owl:PotentialConsequence,
        risk-owl:PotentialImpact,
        risk-owl:PotentialRisk ;
    dct:created "2024-10-21"^^xsd:date ;
    rdfs:isDefinedBy risk-owl: ;
    rdfs:subClassOf risk-owl:EnvironmentalRisk ;
    sw:term_status "accepted"@en ;
    skos:definition "The occurence or potential occurence of floods"@en ;
    skos:prefLabel "Floods"@en .

risk-owl:Fraud a rdfs:Class,
        owl:Class,
        dpv-owl:RiskConcept,
        risk-owl:ConfidentialityConcept,
        risk-owl:PotentialConsequence,
        risk-owl:PotentialRisk,
        risk-owl:PotentialRiskSource ;
    dct:contributor _:Ne22a67b17c7e4a779c30d2864b6a0cee ;
    dct:created "2022-08-17"^^xsd:date ;
    dct:modified "2024-08-16"^^xsd:date ;
    dct:source [ a schema:WebPage ;
            schema:name "ISO/IEC 27005:2018" ;
            schema:url "https://www.iso.org/standard/75281.html" ] ;
    rdfs:isDefinedBy risk-owl: ;
    rdfs:subClassOf risk-owl:MaliciousActivity ;
    sw:term_status "accepted"@en ;
    skos:definition "Concept representing Fraud"@en ;
    skos:prefLabel "Fraud"@en .

risk-owl:GenderDiscrimination a rdfs:Class,
        owl:Class,
        dpv-owl:RiskConcept,
        risk-owl:PotentialConsequence,
        risk-owl:PotentialImpact,
        risk-owl:PotentialRisk ;
    dct:created "2024-09-30"^^xsd:date ;
    rdfs:isDefinedBy risk-owl: ;
    rdfs:subClassOf risk-owl:Sexism ;
    sw:term_status "accepted"@en ;
    skos:definition "Discrimination based on a person's gender identity or gender expression"@en ;
    skos:prefLabel "Gender Discrimination"@en .

risk-owl:GeographicDiscrimination a rdfs:Class,
        owl:Class,
        dpv-owl:RiskConcept,
        risk-owl:PotentialConsequence,
        risk-owl:PotentialImpact,
        risk-owl:PotentialRisk ;
    dct:created "2024-09-30"^^xsd:date ;
    rdfs:isDefinedBy risk-owl: ;
    rdfs:subClassOf risk-owl:Discrimination ;
    sw:term_status "accepted"@en ;
    skos:definition "Discrimination based on a person's geographical origin or residence"@en ;
    skos:prefLabel "Geographic Discrimination"@en .

risk-owl:GroupAttributionBias a rdfs:Class,
        owl:Class,
        dpv-owl:RiskConcept,
        risk-owl:PotentialConsequence,
        risk-owl:PotentialRisk,
        risk-owl:PotentialRiskSource ;
    dct:contributor _:N2e9307242cb14d528effb994db501842,
        _:N9c63c24625fe482386a350b4ea27b4f8,
        _:Ne22a67b17c7e4a779c30d2864b6a0cee ;
    dct:created "2024-09-13"^^xsd:date ;
    dct:source "ISO/IEC 24027:2021"@en ;
    rdfs:isDefinedBy risk-owl: ;
    rdfs:subClassOf risk-owl:CognitiveBias ;
    sw:term_status "accepted"@en ;
    skos:definition "Bias that occurs when a human assumes that what is true for an individual or object is also true for everyone, or all objects, in that group"@en ;
    skos:prefLabel "Group Attribution Bias"@en .

risk-owl:GroupHealthSafety a rdfs:Class,
        owl:Class,
        dpv-owl:RiskConcept,
        risk-owl:PotentialConsequence,
        risk-owl:PotentialImpact,
        risk-owl:PotentialRisk ;
    dct:created "2024-12-01"^^xsd:date ;
    rdfs:isDefinedBy risk-owl: ;
    rdfs:subClassOf risk-owl:GroupRisk,
        risk-owl:HealthSafety ;
    sw:term_status "accepted"@en ;
    skos:definition "Concept representing health & safety of a group or group(s)"@en ;
    skos:prefLabel "Group Health & Safety"@en .

risk-owl:GroupRisk a rdfs:Class,
        owl:Class,
        dpv-owl:RiskConcept,
        risk-owl:PotentialConsequence,
        risk-owl:PotentialImpact,
        risk-owl:PotentialRisk ;
    dct:created "2024-12-17"^^xsd:date ;
    rdfs:isDefinedBy risk-owl: ;
    rdfs:subClassOf risk-owl:SocietalRiskConcept ;
    sw:term_status "accepted"@en ;
    skos:definition "Risks and issues that affect or have the potential to affect groups in society"@en ;
    skos:prefLabel "Societal Risk"@en .

risk-owl:HaltConsequence a rdfs:Class,
        owl:Class,
        risk-owl:RiskControl ;
    dct:contributor _:Ne22a67b17c7e4a779c30d2864b6a0cee ;
    dct:created "2025-01-06"^^xsd:date ;
    rdfs:isDefinedBy risk-owl: ;
    rdfs:subClassOf risk-owl:ConsequenceControl,
        risk-owl:InterruptionControl ;
    sw:term_status "accepted"@en ;
    skos:definition "Control that halts the (ongoing) consequence event or process such that it no longer takes place or is applicable in the context"@en ;
    skos:prefLabel "Halt Consequence"@en .

risk-owl:HaltImpact a rdfs:Class,
        owl:Class,
        risk-owl:RiskControl ;
    dct:contributor _:Ne22a67b17c7e4a779c30d2864b6a0cee ;
    dct:created "2025-01-06"^^xsd:date ;
    rdfs:isDefinedBy risk-owl: ;
    rdfs:subClassOf risk-owl:ImpactControl,
        risk-owl:InterruptionControl ;
    sw:term_status "accepted"@en ;
    skos:definition "Control that halts the (ongoing) impact event or process such that it no longer takes place or is applicable in the context"@en ;
    skos:prefLabel "Halt Impact"@en .

risk-owl:HaltSource a rdfs:Class,
        owl:Class,
        risk-owl:RiskControl ;
    dct:contributor _:Ne22a67b17c7e4a779c30d2864b6a0cee ;
    dct:created "2024-05-19"^^xsd:date ;
    dct:modified "2025-01-06"^^xsd:date ;
    rdfs:isDefinedBy risk-owl: ;
    rdfs:subClassOf risk-owl:InterruptionControl,
        risk-owl:SourceControl ;
    sw:term_status "modified"@en ;
    skos:definition "Control that halts the (ongoing) risk source event or process such that it no longer takes place or is applicable in the context"@en ;
    skos:prefLabel "Halt Source"@en .

risk-owl:Harassment a rdfs:Class,
        owl:Class,
        dpv-owl:RiskConcept,
        risk-owl:PotentialConsequence,
        risk-owl:PotentialImpact,
        risk-owl:PotentialRisk ;
    dct:created "2024-12-17"^^xsd:date ;
    rdfs:isDefinedBy risk-owl: ;
    rdfs:subClassOf risk-owl:Harm,
        risk-owl:Wellbeing ;
    sw:term_status "accepted"@en ;
    skos:definition "Concept representing harassment of individual(s)"@en ;
    skos:prefLabel "Harassment"@en .

risk-owl:Harm a rdfs:Class,
        owl:Class,
        dpv-owl:RiskConcept,
        risk-owl:PotentialConsequence,
        risk-owl:PotentialImpact,
        risk-owl:PotentialRisk ;
    dct:contributor _:Ne22a67b17c7e4a779c30d2864b6a0cee ;
    dct:created "2022-08-13"^^xsd:date ;
    dct:modified "2024-08-16"^^xsd:date ;
    rdfs:isDefinedBy risk-owl: ;
    rdfs:subClassOf risk-owl:HealthSafety,
        risk-owl:IndividualRisk ;
    sw:term_status "accepted"@en ;
    skos:definition "Concept representing Harm to humans"@en ;
    skos:prefLabel "Harm"@en ;
    skos:scopeNote "This concept refers to the general abstract notion of harm"@en .

risk-owl:Health a rdfs:Class,
        owl:Class,
        dpv-owl:RiskConcept,
        risk-owl:PotentialConsequence,
        risk-owl:PotentialImpact,
        risk-owl:PotentialRisk ;
    dct:contributor _:Ne22a67b17c7e4a779c30d2864b6a0cee ;
    dct:created "2024-12-01"^^xsd:date ;
    rdfs:isDefinedBy risk-owl: ;
    rdfs:subClassOf risk-owl:HealthSafety ;
    sw:term_status "accepted"@en ;
    skos:definition "Concept representing health of individual(s), or group(s), or society at large"@en ;
    skos:prefLabel "Health"@en .

risk-owl:HealthSafety a rdfs:Class,
        owl:Class,
        dpv-owl:RiskConcept,
        risk-owl:PotentialConsequence,
        risk-owl:PotentialImpact,
        risk-owl:PotentialRisk ;
    dct:contributor _:N9c63c24625fe482386a350b4ea27b4f8 ;
    dct:created "2024-12-01"^^xsd:date ;
    rdfs:isDefinedBy risk-owl: ;
    rdfs:subClassOf risk-owl:IndividualRisk ;
    sw:term_status "accepted"@en ;
    skos:definition "Concept representing health & safety of individual(s), or group(s), or society at large"@en ;
    skos:prefLabel "Health & Safety"@en .

risk-owl:HighLikelihood a rdfs:Class,
        owl:Class,
        dpv-owl:Likelihood ;
    dct:contributor _:Ne22a67b17c7e4a779c30d2864b6a0cee ;
    dct:created "2022-08-18"^^xsd:date ;
    rdf:value "0.75,xsd:decimal" ;
    rdfs:isDefinedBy risk-owl: ;
    rdfs:subClassOf risk-owl:3LikelihoodLevels,
        risk-owl:5LikelihoodLevels,
        risk-owl:7LikelihoodLevels ;
    sw:term_status "accepted"@en ;
    skos:definition "Level where Likelihood is High"@en ;
    skos:prefLabel "High Likelihood"@en ;
    skos:scopeNote "The suggested quantitative value for this concept is 0.75 on a scale of 0 to 1"@en .

risk-owl:HighRisk a rdfs:Class,
        owl:Class,
        dpv-owl:RiskLevel ;
    dct:contributor _:Ne22a67b17c7e4a779c30d2864b6a0cee ;
    dct:created "2022-08-18"^^xsd:date ;
    rdf:value "0.75,xsd:decimal" ;
    rdfs:isDefinedBy risk-owl: ;
    rdfs:subClassOf risk-owl:3RiskLevels,
        risk-owl:5RiskLevels,
        risk-owl:7RiskLevels ;
    sw:term_status "accepted"@en ;
    skos:definition "Level where Risk is High"@en ;
    skos:prefLabel "High Risk"@en ;
    skos:scopeNote "The suggested quantitative value for this concept is 0.75 on a scale of 0 to 1"@en .

risk-owl:HighSeverity a rdfs:Class,
        owl:Class,
        dpv-owl:Severity ;
    dct:contributor _:Ne22a67b17c7e4a779c30d2864b6a0cee ;
    dct:created "2022-08-18"^^xsd:date ;
    rdf:value "0.75,xsd:decimal" ;
    rdfs:isDefinedBy risk-owl: ;
    rdfs:subClassOf risk-owl:3SeverityLevels,
        risk-owl:5SeverityLevels,
        risk-owl:7SeverityLevels ;
    sw:term_status "accepted"@en ;
    skos:definition "Level where Severity is High"@en ;
    skos:prefLabel "High Severity"@en ;
    skos:scopeNote "The suggested quantitative value for this concept is 0.75 on a scale of 0 to 1"@en .

risk-owl:Homophobia a rdfs:Class,
        owl:Class,
        dpv-owl:RiskConcept,
        risk-owl:PotentialConsequence,
        risk-owl:PotentialImpact,
        risk-owl:PotentialRisk ;
    dct:created "2024-09-30"^^xsd:date ;
    rdfs:isDefinedBy risk-owl: ;
    rdfs:subClassOf risk-owl:SexualOrientationDiscrimination ;
    sw:term_status "accepted"@en ;
    skos:definition "Hostility or prejudice against individuals who are or are perceived to be homosexual"@en ;
    skos:prefLabel "Homophobia"@en .

risk-owl:HumanErrors a rdfs:Class,
        owl:Class,
        dpv-owl:RiskConcept,
        risk-owl:PotentialConsequence,
        risk-owl:PotentialRisk,
        risk-owl:PotentialRiskSource ;
    dct:contributor _:Ne22a67b17c7e4a779c30d2864b6a0cee ;
    dct:created "2022-08-17"^^xsd:date ;
    dct:modified "2024-08-16"^^xsd:date ;
    dct:source [ a schema:WebPage ;
            schema:name "ENISA Reference Incident Classification Taxonomy 2018" ;
            schema:url "https://www.enisa.europa.eu/publications/reference-incident-classification-taxonomy/" ] ;
    rdfs:isDefinedBy risk-owl: ;
    rdfs:subClassOf risk-owl:UserRisks ;
    sw:term_status "accepted"@en ;
    skos:definition "Concept representing activities that are errors caused by humans without intention and which was not caused by following rules or policies or instructions that were not from the person"@en ;
    skos:prefLabel "Human Errors"@en .

risk-owl:HumanOversightIneffective a rdfs:Class,
        owl:Class,
        dpv-owl:RiskConcept,
        risk-owl:PotentialConsequence,
        risk-owl:PotentialRisk,
        risk-owl:PotentialRiskSource ;
    dct:contributor _:N9c63c24625fe482386a350b4ea27b4f8,
        _:Ne22a67b17c7e4a779c30d2864b6a0cee ;
    dct:created "2024-12-01"^^xsd:date ;
    rdfs:isDefinedBy risk-owl: ;
    rdfs:subClassOf risk-owl:OrganisationalManagementRisk ;
    sw:term_status "accepted"@en ;
    skos:definition "Concept representing cases where human oversight is ineffective for the intended effect, such as for when human can observe a problem but cannot do anything about it"@en ;
    skos:prefLabel "Human Oversight Ineffective"@en .

risk-owl:HumanOversightInsufficient a rdfs:Class,
        owl:Class,
        dpv-owl:RiskConcept,
        risk-owl:PotentialConsequence,
        risk-owl:PotentialRisk,
        risk-owl:PotentialRiskSource ;
    dct:contributor _:N9c63c24625fe482386a350b4ea27b4f8,
        _:Ne22a67b17c7e4a779c30d2864b6a0cee ;
    dct:created "2024-12-01"^^xsd:date ;
    rdfs:isDefinedBy risk-owl: ;
    rdfs:subClassOf risk-owl:OrganisationalManagementRisk ;
    sw:term_status "accepted"@en ;
    skos:definition "Concept representing cases where human oversight is insufficient for the intended effect, such as not being capable of identifying a problem"@en ;
    skos:prefLabel "Human Oversight Insufficient"@en .

risk-owl:IdentificationControl a rdfs:Class,
        owl:Class,
        risk-owl:RiskControl ;
    dct:contributor _:N9c63c24625fe482386a350b4ea27b4f8,
        _:Ne22a67b17c7e4a779c30d2864b6a0cee ;
    dct:created "2024-05-19"^^xsd:date ;
    dct:modified "2025-01-06"^^xsd:date ;
    rdfs:isDefinedBy risk-owl: ;
    rdfs:subClassOf risk-owl:MonitorControl ;
    sw:term_status "modified"@en ;
    skos:definition "Control that identifies the characteristics of an event"@en ;
    skos:prefLabel "Identification Control"@en ;
    skos:scopeNote "Identification in the context of an event refers to its characteristics such as likelihood, severity, as well as contextual metrics such as amount of data or power being used, or affected entities or things, and which can be used to categorise the event in terms of risk level or other contextual groupings"@en .

risk-owl:IdentityFraud a rdfs:Class,
        owl:Class,
        dpv-owl:RiskConcept,
        risk-owl:ConfidentialityConcept,
        risk-owl:PotentialConsequence,
        risk-owl:PotentialRisk,
        risk-owl:PotentialRiskSource ;
    dct:contributor _:Ne22a67b17c7e4a779c30d2864b6a0cee ;
    dct:created "2022-08-17"^^xsd:date ;
    dct:modified "2024-08-16"^^xsd:date ;
    dct:source [ a schema:WebPage ;
            schema:name "ENISA Threat Taxonomy 2016" ;
            schema:url "https://www.enisa.europa.eu/topics/threat-risk-management/threats-and-trends/enisa-threat-landscape/threat-taxonomy/view" ] ;
    rdfs:isDefinedBy risk-owl: ;
    rdfs:subClassOf risk-owl:MaliciousActivity ;
    sw:term_status "accepted"@en ;
    skos:definition "Concept representing Identity Fraud"@en ;
    skos:prefLabel "Identity Fraud"@en .

risk-owl:IdentityTheft a rdfs:Class,
        owl:Class,
        dpv-owl:RiskConcept,
        risk-owl:ConfidentialityConcept,
        risk-owl:PotentialConsequence,
        risk-owl:PotentialRisk,
        risk-owl:PotentialRiskSource ;
    dct:contributor _:Ne22a67b17c7e4a779c30d2864b6a0cee ;
    dct:created "2022-08-17"^^xsd:date ;
    dct:modified "2024-08-16"^^xsd:date ;
    dct:source [ a schema:WebPage ;
            schema:name "ENISA Threat Taxonomy 2016" ;
            schema:url "https://www.enisa.europa.eu/topics/threat-risk-management/threats-and-trends/enisa-threat-landscape/threat-taxonomy/view" ] ;
    rdfs:isDefinedBy risk-owl: ;
    rdfs:subClassOf risk-owl:MaliciousActivity ;
    sw:term_status "accepted"@en ;
    skos:definition "Concept representing Identity Theft"@en ;
    skos:prefLabel "Identity Theft"@en .

risk-owl:IdentityVerificationFailure a rdfs:Class,
        owl:Class,
        dpv-owl:RiskConcept,
        risk-owl:PotentialConsequence,
        risk-owl:PotentialImpact,
        risk-owl:PotentialRisk ;
    dct:created "2024-10-21"^^xsd:date ;
    rdfs:isDefinedBy risk-owl: ;
    rdfs:subClassOf risk-owl:ServiceRelatedConsequence ;
    sw:term_status "accepted"@en ;
    skos:definition "Concept representing failure to verify identity"@en ;
    skos:prefLabel "Identity Verification Failure"@en .

risk-owl:IllegalDataProcessing a rdfs:Class,
        owl:Class,
        dpv-owl:RiskConcept,
        risk-owl:PotentialConsequence,
        risk-owl:PotentialRisk ;
    dct:contributor _:Ne22a67b17c7e4a779c30d2864b6a0cee ;
    dct:created "2022-08-17"^^xsd:date ;
    dct:modified "2024-08-16"^^xsd:date ;
    dct:source [ a schema:WebPage ;
            schema:name "ISO/IEC 27005:2018" ;
            schema:url "https://www.iso.org/standard/75281.html" ] ;
    rdfs:isDefinedBy risk-owl: ;
    rdfs:subClassOf risk-owl:LegalComplianceRisk ;
    sw:term_status "accepted"@en ;
    skos:definition "Concept representing Illegal Processing of Data"@en ;
    skos:prefLabel "Illegal Data Processing"@en ;
    skos:scopeNote "This concept was called \"IllegalProcessingData\" in DPV 2.0"@en .

risk-owl:ImpactControl a rdfs:Class,
        owl:Class,
        risk-owl:RiskControl ;
    dct:contributor _:Ne22a67b17c7e4a779c30d2864b6a0cee ;
    dct:created "2024-05-19"^^xsd:date ;
    dct:modified "2025-01-06"^^xsd:date ;
    rdfs:isDefinedBy risk-owl: ;
    rdfs:subClassOf risk-owl:RiskControl ;
    sw:term_status "modified"@en ;
    skos:definition "Risk Mitigation Measure that controls Impacts"@en ;
    skos:prefLabel "Impact Control"@en .

risk-owl:ImplicitBias a rdfs:Class,
        owl:Class,
        dpv-owl:RiskConcept,
        risk-owl:PotentialConsequence,
        risk-owl:PotentialRisk,
        risk-owl:PotentialRiskSource ;
    dct:contributor _:N2e9307242cb14d528effb994db501842,
        _:N9c63c24625fe482386a350b4ea27b4f8,
        _:Ne22a67b17c7e4a779c30d2864b6a0cee ;
    dct:created "2024-09-13"^^xsd:date ;
    dct:source "ISO/IEC 24027:2021"@en ;
    rdfs:isDefinedBy risk-owl: ;
    rdfs:subClassOf risk-owl:CognitiveBias ;
    sw:term_status "accepted"@en ;
    skos:definition "Bias that occurs when a human makes an association or assumption based on their mental models and memories"@en ;
    skos:prefLabel "Implicit Bias"@en .

risk-owl:InGroupBias a rdfs:Class,
        owl:Class,
        dpv-owl:RiskConcept,
        risk-owl:PotentialConsequence,
        risk-owl:PotentialRisk,
        risk-owl:PotentialRiskSource ;
    dct:contributor _:N2e9307242cb14d528effb994db501842,
        _:N9c63c24625fe482386a350b4ea27b4f8,
        _:Ne22a67b17c7e4a779c30d2864b6a0cee ;
    dct:created "2024-09-13"^^xsd:date ;
    dct:source "ISO/IEC 24027:2021"@en ;
    rdfs:isDefinedBy risk-owl: ;
    rdfs:subClassOf risk-owl:CognitiveBias ;
    sw:term_status "accepted"@en ;
    skos:definition "Bias that occurs when showing partiality to one's own group or own characteristics"@en ;
    skos:prefLabel "In-Group Bias"@en .

risk-owl:InabilityToEnterIntoContract a rdfs:Class,
        owl:Class,
        dpv-owl:RiskConcept,
        risk-owl:PotentialConsequence,
        risk-owl:PotentialImpact,
        risk-owl:PotentialRisk ;
    dct:created "2024-10-21"^^xsd:date ;
    rdfs:isDefinedBy risk-owl: ;
    rdfs:subClassOf risk-owl:ServiceRelatedConsequence ;
    sw:term_status "accepted"@en ;
    skos:definition "Concept representing inability to enter into contract"@en ;
    skos:prefLabel "Inability to Enter Into Contract"@en .

risk-owl:InabilityToEstablishLegalClaims a rdfs:Class,
        owl:Class,
        dpv-owl:RiskConcept,
        risk-owl:PotentialConsequence,
        risk-owl:PotentialImpact,
        risk-owl:PotentialRisk ;
    dct:created "2024-10-21"^^xsd:date ;
    rdfs:isDefinedBy risk-owl: ;
    rdfs:subClassOf risk-owl:ServiceRelatedConsequence ;
    sw:term_status "accepted"@en ;
    skos:definition "Concept representing inability to establish legal claims"@en ;
    skos:prefLabel "Inability to Establish Legal Claims"@en .

risk-owl:InabilityToFulfillLegalObligations a rdfs:Class,
        owl:Class,
        dpv-owl:RiskConcept,
        risk-owl:PotentialConsequence,
        risk-owl:PotentialImpact,
        risk-owl:PotentialRisk ;
    dct:created "2024-10-21"^^xsd:date ;
    rdfs:isDefinedBy risk-owl: ;
    rdfs:subClassOf risk-owl:ServiceRelatedConsequence ;
    sw:term_status "accepted"@en ;
    skos:definition "Concept representing inability to fulfill legal obligations"@en ;
    skos:prefLabel "Inability to Fulfill Legal Obligations"@en .

risk-owl:InabilityToProcessPayments a rdfs:Class,
        owl:Class,
        dpv-owl:RiskConcept,
        risk-owl:PotentialConsequence,
        risk-owl:PotentialImpact,
        risk-owl:PotentialRisk ;
    dct:created "2024-10-21"^^xsd:date ;
    rdfs:isDefinedBy risk-owl: ;
    rdfs:subClassOf risk-owl:ServiceRelatedConsequence ;
    sw:term_status "accepted"@en ;
    skos:definition "Concept representing inability to process payments"@en ;
    skos:prefLabel "Inability to Process Payments"@en .

risk-owl:InabilityToProtectVitalInterests a rdfs:Class,
        owl:Class,
        dpv-owl:RiskConcept,
        risk-owl:PotentialConsequence,
        risk-owl:PotentialImpact,
        risk-owl:PotentialRisk ;
    dct:created "2024-10-21"^^xsd:date ;
    rdfs:isDefinedBy risk-owl: ;
    rdfs:subClassOf risk-owl:ServiceRelatedConsequence ;
    sw:term_status "accepted"@en ;
    skos:definition "Concept representing inability to protect vital interests"@en ;
    skos:prefLabel "Inability to Protect Vital Interests"@en .

risk-owl:InabilityToProvideHealthCare a rdfs:Class,
        owl:Class,
        dpv-owl:RiskConcept,
        risk-owl:PotentialConsequence,
        risk-owl:PotentialImpact,
        risk-owl:PotentialRisk ;
    dct:created "2024-10-21"^^xsd:date ;
    rdfs:isDefinedBy risk-owl: ;
    rdfs:subClassOf risk-owl:ServiceRelatedConsequence ;
    sw:term_status "accepted"@en ;
    skos:definition "Concept representing inability to provide health care"@en ;
    skos:prefLabel "Inability to Provide Health Care"@en .

risk-owl:Incident a rdfs:Class,
        owl:Class ;
    dct:contributor _:N59852c09189e47bd989757f1615f7bdf,
        _:N9c63c24625fe482386a350b4ea27b4f8,
        _:Naa42ed8e13734cd887c18487fe7930ec,
        _:Ne22a67b17c7e4a779c30d2864b6a0cee ;
    dct:created "2024-02-14"^^xsd:date ;
    dct:modified "2024-08-16"^^xsd:date ;
    vann:example dex-owl:E0069,
        dex-owl:E0070 ;
    rdfs:isDefinedBy risk-owl: ;
    rdfs:subClassOf dpv-owl:RiskConcept ;
    sw:term_status "accepted"@en ;
    skos:definition "An actual or occured event"@en ;
    skos:prefLabel "Incident"@en ;
    skos:scopeNote "Incident is realised or materialised risk"@en .

risk-owl:IncidentAssessmentReport a rdfs:Class,
        owl:Class ;
    dct:created "2024-05-19"^^xsd:date ;
    rdfs:isDefinedBy risk-owl: ;
    rdfs:subClassOf risk-owl:IncidentReport ;
    sw:term_status "accepted"@en ;
    skos:definition "A report describing the assessment of an incident in terms of its effects or impacts"@en ;
    skos:prefLabel "Incident Assessment Report"@en .

risk-owl:IncidentConcluded a rdfs:Class,
        owl:Class,
        risk-owl:IncidentStatus ;
    dct:contributor _:Ne22a67b17c7e4a779c30d2864b6a0cee ;
    dct:created "2024-02-14"^^xsd:date ;
    rdfs:isDefinedBy risk-owl: ;
    rdfs:subClassOf risk-owl:IncidentStatus ;
    sw:term_status "accepted"@en ;
    skos:definition "The incident has stopped or finished or concluded without any active mitigation and with a low likelihood of resuming or recurring"@en ;
    skos:prefLabel "Incident Concluded"@en .

risk-owl:IncidentConcludingReport a rdfs:Class,
        owl:Class ;
    dct:created "2024-05-19"^^xsd:date ;
    rdfs:isDefinedBy risk-owl: ;
    rdfs:subClassOf risk-owl:IncidentReport ;
    sw:term_status "accepted"@en ;
    skos:definition "A report describing the conclusion of an investigation regarding a Incident where all relevant facts are known"@en ;
    skos:prefLabel "Incident Concluding Report"@en .

risk-owl:IncidentDetectionReport a rdfs:Class,
        owl:Class ;
    dct:created "2024-05-19"^^xsd:date ;
    rdfs:isDefinedBy risk-owl: ;
    rdfs:subClassOf risk-owl:IncidentReport ;
    sw:term_status "accepted"@en ;
    skos:definition "A report describing the detection of a Incident"@en ;
    skos:prefLabel "Incident Detection Report"@en .

risk-owl:IncidentHalted a rdfs:Class,
        owl:Class,
        risk-owl:IncidentStatus ;
    dct:contributor _:Ne22a67b17c7e4a779c30d2864b6a0cee ;
    dct:created "2024-02-14"^^xsd:date ;
    rdfs:isDefinedBy risk-owl: ;
    rdfs:subClassOf risk-owl:IncidentStatus ;
    sw:term_status "accepted"@en ;
    skos:definition "The incident has halted or paused with a high  likelihood of resuming or recurring"@en ;
    skos:prefLabel "Incident Halted"@en .

risk-owl:IncidentHandlingReport a rdfs:Class,
        owl:Class ;
    dct:created "2024-05-19"^^xsd:date ;
    rdfs:isDefinedBy risk-owl: ;
    rdfs:subClassOf risk-owl:IncidentReport ;
    sw:term_status "accepted"@en ;
    skos:definition "A report describing the response to or handling of an incident regarding the mitigation of its effects and the prevention of its recurrence"@en ;
    skos:prefLabel "Incident Handling Report"@en .

risk-owl:IncidentIdentifier a rdfs:Class,
        owl:Class ;
    dct:created "2024-05-19"^^xsd:date ;
    rdfs:isDefinedBy risk-owl: ;
    rdfs:subClassOf rdfs:Class ;
    sw:term_status "accepted"@en ;
    skos:definition "Identifier associated with an incident"@en ;
    skos:prefLabel "Incident Identifier"@en .

risk-owl:IncidentImpactAssessment a rdfs:Class,
        owl:Class ;
    dct:contributor _:Ne22a67b17c7e4a779c30d2864b6a0cee ;
    dct:created "2024-05-19"^^xsd:date ;
    rdfs:isDefinedBy risk-owl: ;
    rdfs:subClassOf dpv-owl:ImpactAssessment ;
    sw:term_status "accepted"@en ;
    skos:definition "An impact assessment associated with a incident"@en ;
    skos:prefLabel "Incident Impact Assessment"@en .

risk-owl:IncidentInvestigationCompleted a rdfs:Class,
        owl:Class,
        risk-owl:IncidentInvestigationStatus ;
    dct:contributor _:Ne22a67b17c7e4a779c30d2864b6a0cee ;
    dct:created "2024-12-01"^^xsd:date ;
    rdfs:isDefinedBy risk-owl: ;
    rdfs:subClassOf risk-owl:IncidentInvestigationStatus ;
    sw:term_status "accepted"@en ;
    skos:definition "Status indicating the investigation has been completed and findings are available"@en ;
    skos:prefLabel "Incident Investigation Completed"@en .

risk-owl:IncidentInvestigationNotStarted a rdfs:Class,
        owl:Class,
        risk-owl:IncidentInvestigationStatus ;
    dct:contributor _:Ne22a67b17c7e4a779c30d2864b6a0cee ;
    dct:created "2024-12-01"^^xsd:date ;
    rdfs:isDefinedBy risk-owl: ;
    rdfs:subClassOf risk-owl:IncidentInvestigationStatus ;
    sw:term_status "accepted"@en ;
    skos:definition "Status indicating the investigation has not yet been started"@en ;
    skos:prefLabel "Incident Investigation Not Started"@en .

risk-owl:IncidentInvestigationOngoing a rdfs:Class,
        owl:Class,
        risk-owl:IncidentInvestigationStatus ;
    dct:contributor _:Ne22a67b17c7e4a779c30d2864b6a0cee ;
    dct:created "2024-12-01"^^xsd:date ;
    rdfs:isDefinedBy risk-owl: ;
    rdfs:subClassOf risk-owl:IncidentInvestigationStatus ;
    sw:term_status "accepted"@en ;
    skos:definition "Status indicating the investigation is ongoing"@en ;
    skos:prefLabel "Incident Investigation Ongoing"@en .

risk-owl:IncidentInvestigationPreliminary a rdfs:Class,
        owl:Class,
        risk-owl:IncidentInvestigationStatus ;
    dct:contributor _:Ne22a67b17c7e4a779c30d2864b6a0cee ;
    dct:created "2024-12-01"^^xsd:date ;
    rdfs:isDefinedBy risk-owl: ;
    rdfs:subClassOf risk-owl:IncidentInvestigationStatus ;
    sw:term_status "accepted"@en ;
    skos:definition "Status indicating the investigation is at a preliminary stage with limited findings"@en ;
    skos:prefLabel "Incident Investigation Preliminary"@en .

risk-owl:IncidentInvestigationStatus a rdfs:Class,
        owl:Class ;
    dct:contributor _:Ne22a67b17c7e4a779c30d2864b6a0cee ;
    dct:created "2024-12-01"^^xsd:date ;
    rdfs:isDefinedBy risk-owl: ;
    rdfs:subClassOf dpv-owl:Status ;
    sw:term_status "accepted"@en ;
    skos:definition "Status associated with investigation of an incident"@en ;
    skos:prefLabel "Incident Investigation Status"@en .

risk-owl:IncidentMitigated a rdfs:Class,
        owl:Class,
        risk-owl:IncidentStatus ;
    dct:contributor _:Ne22a67b17c7e4a779c30d2864b6a0cee ;
    dct:created "2024-02-14"^^xsd:date ;
    rdfs:isDefinedBy risk-owl: ;
    rdfs:subClassOf risk-owl:IncidentStatus ;
    sw:term_status "accepted"@en ;
    skos:definition "The incident has been mitigated against future recurrences i.e. a measure has been applied to prevent the same or similar incident from recurring"@en ;
    skos:prefLabel "Incident Mitigated"@en .

risk-owl:IncidentMitigationMeasure a rdfs:Class,
        owl:Class ;
    dct:created "2024-05-19"^^xsd:date ;
    rdfs:isDefinedBy risk-owl: ;
    rdfs:subClassOf dpv-owl:RiskMitigationMeasure ;
    sw:term_status "accepted"@en ;
    skos:definition "A mitigation measure taken in response specifically to mitigate an incident and prevent it from occurring again"@en ;
    skos:prefLabel "Incident Mitigation Measure"@en .

risk-owl:IncidentNearMiss a rdfs:Class,
        owl:Class,
        risk-owl:IncidentStatus ;
    dct:contributor _:Ne22a67b17c7e4a779c30d2864b6a0cee ;
    dct:created "2024-02-14"^^xsd:date ;
    rdfs:isDefinedBy risk-owl: ;
    rdfs:subClassOf risk-owl:IncidentStatus ;
    sw:term_status "accepted"@en ;
    skos:definition "The state where an incident was almost successful in taking place i.e. \"it came very close\""@en ;
    skos:prefLabel "Incident Near Miss"@en .

risk-owl:IncidentNotice a rdfs:Class,
        owl:Class ;
    dct:created "2024-05-19"^^xsd:date ;
    rdfs:isDefinedBy risk-owl: ;
    rdfs:subClassOf dpv-owl:Notice ;
    sw:term_status "accepted"@en ;
    skos:definition "Notice associated with an Incident"@en ;
    skos:prefLabel "Incident Notice"@en .

risk-owl:IncidentOngoing a rdfs:Class,
        owl:Class,
        risk-owl:IncidentStatus ;
    dct:contributor _:Ne22a67b17c7e4a779c30d2864b6a0cee ;
    dct:created "2024-02-14"^^xsd:date ;
    rdfs:isDefinedBy risk-owl: ;
    rdfs:subClassOf risk-owl:IncidentStatus ;
    sw:term_status "accepted"@en ;
    skos:definition "The incident is ongoing i.e. still active"@en ;
    skos:prefLabel "Incident Ongoing"@en .

risk-owl:IncidentOngoingReport a rdfs:Class,
        owl:Class ;
    dct:created "2024-05-19"^^xsd:date ;
    rdfs:isDefinedBy risk-owl: ;
    rdfs:subClassOf risk-owl:IncidentReport ;
    sw:term_status "accepted"@en ;
    skos:definition "A report describing on ongoing investigation regarding a Incident where facts and extent of the investigation are being investigated"@en ;
    skos:prefLabel "Incident Ongoing Report"@en .

risk-owl:IncidentPreliminaryReport a rdfs:Class,
        owl:Class ;
    dct:created "2024-05-19"^^xsd:date ;
    rdfs:isDefinedBy risk-owl: ;
    rdfs:subClassOf risk-owl:IncidentReport ;
    sw:term_status "accepted"@en ;
    skos:definition "A report describing the preliminary investigation regarding a Incident where the complete facts or extent of the incident may not be known"@en ;
    skos:prefLabel "Incident Preliminary Report"@en .

risk-owl:IncidentRegister a rdfs:Class,
        owl:Class ;
    dct:contributor _:Ne22a67b17c7e4a779c30d2864b6a0cee ;
    dct:created "2024-05-19"^^xsd:date ;
    rdfs:isDefinedBy risk-owl: ;
    rdfs:subClassOf dpv-owl:RecordsOfActivities ;
    sw:term_status "accepted"@en ;
    skos:definition "A register recording incidentes, their reports, notifications, and other related activities"@en ;
    skos:prefLabel "Incident Register"@en .

risk-owl:IncidentReport a rdfs:Class,
        owl:Class ;
    dct:created "2024-05-19"^^xsd:date ;
    rdfs:isDefinedBy risk-owl: ;
    rdfs:subClassOf dpv-owl:RecordsOfActivities ;
    sw:term_status "accepted"@en ;
    skos:definition "Documented information about an incident, its handling, assessments,and notifications"@en ;
    skos:prefLabel "Incident Report"@en .

risk-owl:IncidentStatus a rdfs:Class,
        owl:Class ;
    dct:contributor _:Ne22a67b17c7e4a779c30d2864b6a0cee ;
    dct:created "2024-02-14"^^xsd:date ;
    vann:example dex-owl:E0069 ;
    rdfs:isDefinedBy risk-owl: ;
    rdfs:subClassOf dpv-owl:Status ;
    sw:term_status "accepted"@en ;
    skos:definition "Status associated with an incident"@en ;
    skos:prefLabel "Incident Status"@en .

risk-owl:IncidentStatusUnknown a rdfs:Class,
        owl:Class,
        risk-owl:IncidentStatus ;
    dct:contributor _:Ne22a67b17c7e4a779c30d2864b6a0cee ;
    dct:created "2024-02-14"^^xsd:date ;
    rdfs:isDefinedBy risk-owl: ;
    rdfs:subClassOf risk-owl:IncidentStatus ;
    sw:term_status "accepted"@en ;
    skos:definition "The status of a incident is unknown"@en ;
    skos:prefLabel "Incident Status Unknown"@en .

risk-owl:IncidentSuspected a rdfs:Class,
        owl:Class,
        risk-owl:IncidentStatus ;
    dct:contributor _:Ne22a67b17c7e4a779c30d2864b6a0cee ;
    dct:created "2024-02-14"^^xsd:date ;
    rdfs:isDefinedBy risk-owl: ;
    rdfs:subClassOf risk-owl:IncidentStatus ;
    sw:term_status "accepted"@en ;
    skos:definition "The state where a incident is suspected, but has not yet been confirmed. This can be due to lack of information, or because the process of detection and investigation is still ongoing"@en ;
    skos:prefLabel "Incident Suspected"@en .

risk-owl:IncidentSuspectedReport a rdfs:Class,
        owl:Class ;
    dct:created "2024-05-19"^^xsd:date ;
    rdfs:isDefinedBy risk-owl: ;
    rdfs:subClassOf risk-owl:IncidentReport ;
    sw:term_status "accepted"@en ;
    skos:definition "A report describing the suspicion of an incident in the past or occuring"@en ;
    skos:prefLabel "Incident Suspected Report"@en .

risk-owl:IncidentTerminated a rdfs:Class,
        owl:Class,
        risk-owl:IncidentStatus ;
    dct:contributor _:Ne22a67b17c7e4a779c30d2864b6a0cee ;
    dct:created "2024-02-14"^^xsd:date ;
    rdfs:isDefinedBy risk-owl: ;
    rdfs:subClassOf risk-owl:IncidentStatus ;
    sw:term_status "accepted"@en ;
    skos:definition "The incident has been stopped or terminated through the use of a mitigation or deterrent measure with a low likelihood of resuming or recurring"@en ;
    skos:prefLabel "Incident Terminated"@en .

risk-owl:IndirectDiscrimination a rdfs:Class,
        owl:Class,
        dpv-owl:RiskConcept,
        risk-owl:PotentialConsequence,
        risk-owl:PotentialImpact,
        risk-owl:PotentialRisk ;
    dct:created "2024-09-30"^^xsd:date ;
    rdfs:isDefinedBy risk-owl: ;
    rdfs:subClassOf risk-owl:Discrimination ;
    sw:term_status "accepted"@en ;
    skos:definition "Occurs when an apparently neutral provision, criterion, or practice puts individuals of a certain group at a disadvantage compared to others, unless it can be objectively justified"@en ;
    skos:prefLabel "Indirect Discrimination"@en .

risk-owl:IndividualHealthSafety a rdfs:Class,
        owl:Class,
        dpv-owl:RiskConcept,
        risk-owl:PotentialConsequence,
        risk-owl:PotentialImpact,
        risk-owl:PotentialRisk ;
    dct:created "2022-08-17"^^xsd:date ;
    dct:modified "2024-12-01"^^xsd:date ;
    rdfs:isDefinedBy risk-owl: ;
    rdfs:subClassOf risk-owl:HealthSafety,
        risk-owl:IndividualRisk ;
    sw:term_status "modified"@en ;
    skos:definition "Concept representing health & safety of individual(s)"@en ;
    skos:prefLabel "Individual Health & Safety"@en .

risk-owl:IndividualRisk a rdfs:Class,
        owl:Class,
        dpv-owl:RiskConcept,
        risk-owl:PotentialConsequence,
        risk-owl:PotentialImpact,
        risk-owl:PotentialRisk ;
    dct:created "2024-12-17"^^xsd:date ;
    rdfs:isDefinedBy risk-owl: ;
    rdfs:subClassOf risk-owl:SocietalRiskConcept ;
    sw:term_status "accepted"@en ;
    skos:definition "Risks and issues that affect or have the potential to affect specific individuals"@en ;
    skos:prefLabel "Individual Risk"@en .

risk-owl:InformativenessBias a rdfs:Class,
        owl:Class,
        dpv-owl:RiskConcept,
        risk-owl:PotentialConsequence,
        risk-owl:PotentialRisk,
        risk-owl:PotentialRiskSource ;
    dct:contributor _:N2e9307242cb14d528effb994db501842,
        _:N9c63c24625fe482386a350b4ea27b4f8,
        _:Ne22a67b17c7e4a779c30d2864b6a0cee ;
    dct:created "2024-09-13"^^xsd:date ;
    dct:source "ISO/IEC 24027:2021"@en ;
    rdfs:isDefinedBy risk-owl: ;
    rdfs:subClassOf risk-owl:DataBias ;
    sw:term_status "accepted"@en ;
    skos:definition "Bias that occurs when the mapping between inputs present in the data and outputs are more difficult to identify for some group"@en ;
    skos:prefLabel "Informativeness Bias"@en .

risk-owl:Injury a rdfs:Class,
        owl:Class,
        dpv-owl:RiskConcept,
        risk-owl:PotentialConsequence,
        risk-owl:PotentialImpact,
        risk-owl:PotentialRisk ;
    dct:contributor _:Ne22a67b17c7e4a779c30d2864b6a0cee ;
    dct:created "2022-08-17"^^xsd:date ;
    dct:modified "2024-08-16"^^xsd:date ;
    dct:source [ a schema:WebPage ;
            schema:name "ISO/IEC 27005:2018" ;
            schema:url "https://www.iso.org/standard/75281.html" ] ;
    rdfs:isDefinedBy risk-owl: ;
    rdfs:subClassOf risk-owl:Harm,
        risk-owl:PhysicalSafety ;
    sw:term_status "accepted"@en ;
    skos:definition "Concept representing Injury"@en ;
    skos:prefLabel "Injury"@en .

risk-owl:InstructionsIncorrect a rdfs:Class,
        owl:Class,
        dpv-owl:RiskConcept,
        risk-owl:PotentialConsequence,
        risk-owl:PotentialRisk,
        risk-owl:PotentialRiskSource ;
    dct:contributor _:N9c63c24625fe482386a350b4ea27b4f8,
        _:Ne22a67b17c7e4a779c30d2864b6a0cee ;
    dct:created "2024-12-01"^^xsd:date ;
    rdfs:isDefinedBy risk-owl: ;
    rdfs:subClassOf risk-owl:OrganisationalManagementRisk ;
    sw:term_status "accepted"@en ;
    skos:definition "Concept representing cases where instructions are incorrect for achieving the intended effect"@en ;
    skos:prefLabel "Instructions Incorrect"@en .

risk-owl:InstructionsInsufficient a rdfs:Class,
        owl:Class,
        dpv-owl:RiskConcept,
        risk-owl:PotentialConsequence,
        risk-owl:PotentialRisk,
        risk-owl:PotentialRiskSource ;
    dct:contributor _:N9c63c24625fe482386a350b4ea27b4f8,
        _:Ne22a67b17c7e4a779c30d2864b6a0cee ;
    dct:created "2024-12-01"^^xsd:date ;
    rdfs:isDefinedBy risk-owl: ;
    rdfs:subClassOf risk-owl:OrganisationalManagementRisk ;
    sw:term_status "accepted"@en ;
    skos:definition "Concept representing cases where instructions are not sufficient for the intended effect"@en ;
    skos:prefLabel "Instructions Insufficient"@en .

risk-owl:IntegrityBreach a rdfs:Class,
        owl:Class,
        dpv-owl:RiskConcept,
        risk-owl:IntegrityConcept,
        risk-owl:PotentialConsequence,
        risk-owl:PotentialRisk,
        risk-owl:PotentialRiskSource ;
    dct:created "2024-12-17"^^xsd:date ;
    rdfs:isDefinedBy risk-owl: ;
    rdfs:subClassOf risk-owl:DataBreach ;
    sw:term_status "accepted"@en ;
    skos:definition "Concept representing a breach of integrity"@en ;
    skos:prefLabel "Integrity Breachj"@en .

risk-owl:IntegrityConcept a rdfs:Class,
        owl:Class ;
    dct:contributor _:Ne22a67b17c7e4a779c30d2864b6a0cee ;
    dct:created "2024-09-29"^^xsd:date ;
    rdfs:isDefinedBy risk-owl: ;
    rdfs:subClassOf dpv-owl:RiskConcept ;
    sw:term_status "accepted"@en ;
    skos:definition "Indicates a concept is relevant to 'Integrity' in CIA InfoSec model"@en ;
    skos:prefLabel "Integrity Concept"@en ;
    skos:scopeNote "This concept allows indicating the applicability of Integrity dimension to concepts whether they are a risk source, risk, consequence, or impact"@en .

risk-owl:IntegrityIncident a rdfs:Class,
        owl:Class ;
    dct:created "2024-05-19"^^xsd:date ;
    rdfs:isDefinedBy risk-owl: ;
    rdfs:subClassOf risk-owl:Incident ;
    sw:term_status "accepted"@en ;
    skos:definition "Incident where the integrity of information or system has been affected"@en ;
    skos:prefLabel "Integrity Incident"@en .

risk-owl:IntentionalMisuse a rdfs:Class,
        owl:Class,
        dpv-owl:RiskConcept,
        risk-owl:PotentialConsequence,
        risk-owl:PotentialRisk,
        risk-owl:PotentialRiskSource ;
    dct:created "2024-12-17"^^xsd:date ;
    rdfs:isDefinedBy risk-owl: ;
    rdfs:subClassOf risk-owl:Misuse ;
    sw:term_status "accepted"@en ;
    skos:definition "Concept represent an intentional misuse (of something)"@en ;
    skos:prefLabel "Intentional Misuse"@en .

risk-owl:InterceptCommunications a rdfs:Class,
        owl:Class,
        dpv-owl:RiskConcept,
        risk-owl:ConfidentialityConcept,
        risk-owl:PotentialConsequence,
        risk-owl:PotentialRisk,
        risk-owl:PotentialRiskSource ;
    dct:contributor _:Ne22a67b17c7e4a779c30d2864b6a0cee ;
    dct:created "2022-08-17"^^xsd:date ;
    dct:modified "2024-08-16"^^xsd:date ;
    dct:source [ a schema:WebPage ;
            schema:name "ISO/IEC 27005:2018" ;
            schema:url "https://www.iso.org/standard/75281.html" ] ;
    rdfs:isDefinedBy risk-owl: ;
    rdfs:subClassOf risk-owl:MaliciousActivity ;
    sw:term_status "modified"@en ;
    skos:definition "Concept representing Interception of Communications"@en ;
    skos:prefLabel "Intercept Communications"@en ;
    skos:scopeNote "This concept was called \"InterceptionCommunications\" in DPV 2.0"@en .

risk-owl:InterruptionControl a rdfs:Class,
        owl:Class,
        risk-owl:RiskControl ;
    dct:contributor _:N9c63c24625fe482386a350b4ea27b4f8,
        _:Ne22a67b17c7e4a779c30d2864b6a0cee ;
    dct:created "2025-01-06"^^xsd:date ;
    rdfs:isDefinedBy risk-owl: ;
    rdfs:subClassOf risk-owl:ReductionControl ;
    sw:term_status "accepted"@en ;
    skos:definition "Control that interrupts an event without removing the possibility for it to be resumed and where the aim is to stop the event"@en ;
    skos:prefLabel "Interruption Control"@en ;
    skos:scopeNote "Interruption refers to the event being temporarily halted, such as an emergency measure while further suitable measures are identified and put in place. To indicate stopping the event completely rather than a temporary interruption, see risk:RemediationControl which fixes the underlying issue and risk:EliminationEvent which prevents the event from occuring"@en .

risk-owl:InterventionControl a rdfs:Class,
        owl:Class,
        risk-owl:RiskControl ;
    dct:contributor _:Ne22a67b17c7e4a779c30d2864b6a0cee ;
    dct:created "2025-01-06"^^xsd:date ;
    rdfs:isDefinedBy risk-owl: ;
    rdfs:subClassOf risk-owl:ReductionControl ;
    sw:term_status "accepted"@en ;
    skos:definition "Control that intervenes in the operations of the event to change some context with the aim of changing the event or the effects"@en ;
    skos:prefLabel "Intervention Control"@en ;
    skos:scopeNote "Intervention implies taking steps to resolve the effects or to prevent further escalation while the event is still ongoing. For halting the event, see risk:InterruptionControl, for recovering and undoing the effects, see risk:RecoveryControl and risk:ReversalControl. Intervention is a temporary or stop-gap measure which is used while the event is ongoing to prevent it from escalating or creating additional issues"@en .

risk-owl:InvestigationControl a rdfs:Class,
        owl:Class,
        risk-owl:RiskControl ;
    dct:contributor _:Ne22a67b17c7e4a779c30d2864b6a0cee ;
    dct:created "2025-01-06"^^xsd:date ;
    rdfs:isDefinedBy risk-owl: ;
    rdfs:subClassOf risk-owl:ReactiveControl ;
    sw:term_status "accepted"@en ;
    skos:definition "Control that identifies information through an investigative process about an event and its effects after it has occured"@en ;
    skos:prefLabel "Investigation Control"@en ;
    skos:scopeNote "Investigative controls are used to identify information about an event and its effects which can be used to identify further effective measures to address them, and to identify processes to remedy and recover from it. Investigation control therefore is focused on analysis of an event after its occurence with the goal of identifying applicability and effectiveness of other controls to address it"@en .

risk-owl:JudicialCosts a rdfs:Class,
        owl:Class,
        dpv-owl:RiskConcept,
        risk-owl:PotentialConsequence,
        risk-owl:PotentialImpact,
        risk-owl:PotentialRisk ;
    dct:created "2024-12-17"^^xsd:date ;
    rdfs:isDefinedBy risk-owl: ;
    rdfs:subClassOf risk-owl:FinancialLoss ;
    sw:term_status "accepted"@en ;
    skos:definition "Something that involves or causes judicial costs to be paid"@en ;
    skos:prefLabel "Judicial Costs"@en .

risk-owl:JudicialPenalty a rdfs:Class,
        owl:Class,
        dpv-owl:RiskConcept,
        risk-owl:PotentialConsequence,
        risk-owl:PotentialImpact,
        risk-owl:PotentialRisk ;
    dct:created "2024-12-17"^^xsd:date ;
    rdfs:isDefinedBy risk-owl: ;
    rdfs:subClassOf risk-owl:FinancialLoss ;
    sw:term_status "accepted"@en ;
    skos:definition "Something that involves or causes judicial penalties to be paid"@en ;
    skos:prefLabel "Judicial Penalty"@en .

risk-owl:LackOfSystemTransparency a rdfs:Class,
        owl:Class,
        dpv-owl:RiskConcept,
        risk-owl:PotentialConsequence,
        risk-owl:PotentialRisk,
        risk-owl:PotentialRiskSource ;
    dct:contributor _:N9c63c24625fe482386a350b4ea27b4f8,
        _:Ne22a67b17c7e4a779c30d2864b6a0cee ;
    dct:created "2024-12-01"^^xsd:date ;
    rdfs:isDefinedBy risk-owl: ;
    rdfs:subClassOf risk-owl:OrganisationalManagementRisk ;
    sw:term_status "accepted"@en ;
    skos:definition "Concept representing lack of transpareny to humans related to the operation of a system"@en ;
    skos:prefLabel "Lack Of System Transparency"@en .

risk-owl:LanguageDiscrimination a rdfs:Class,
        owl:Class,
        dpv-owl:RiskConcept,
        risk-owl:PotentialConsequence,
        risk-owl:PotentialImpact,
        risk-owl:PotentialRisk ;
    dct:created "2024-09-30"^^xsd:date ;
    rdfs:isDefinedBy risk-owl: ;
    rdfs:subClassOf risk-owl:Discrimination ;
    sw:term_status "accepted"@en ;
    skos:definition "Discrimination based on a person's language, often linked to national origin or ethnicity"@en ;
    skos:prefLabel "Language Discrimination"@en .

risk-owl:LegalComplianceRisk a rdfs:Class,
        owl:Class,
        dpv-owl:RiskConcept,
        risk-owl:PotentialConsequence,
        risk-owl:PotentialRisk,
        risk-owl:PotentialRiskSource ;
    dct:created "2024-12-17"^^xsd:date ;
    rdfs:isDefinedBy risk-owl: ;
    rdfs:subClassOf risk-owl:LegalRiskConcept ;
    sw:term_status "accepted"@en ;
    skos:definition "Risks and consequences regarding legal compliance and its violation"@en ;
    skos:prefLabel "Legal Compliance Risk"@en .

risk-owl:LegalRiskConcept a rdfs:Class,
        owl:Class,
        dpv-owl:RiskConcept,
        risk-owl:PotentialConsequence,
        risk-owl:PotentialImpact,
        risk-owl:PotentialRisk,
        risk-owl:PotentialRiskSource ;
    dct:created "2024-10-21"^^xsd:date ;
    rdfs:isDefinedBy risk-owl: ;
    rdfs:subClassOf dpv-owl:RiskConcept ;
    sw:term_status "accepted"@en ;
    skos:definition "Risk concepts, including any potential risk sources, consequences, or impacts, that are legal in nature or relate to a legal system or process"@en ;
    skos:prefLabel "Legal Risk Concept"@en ;
    skos:scopeNote "Legal in this context refers exclusively to the law applied within a jurisdiction and does not include internal policies or rules within an organisation"@en .

risk-owl:LegalSupportLimited a rdfs:Class,
        owl:Class,
        dpv-owl:RiskConcept,
        risk-owl:PotentialConsequence,
        risk-owl:PotentialImpact,
        risk-owl:PotentialRisk ;
    dct:created "2024-10-21"^^xsd:date ;
    rdfs:isDefinedBy risk-owl: ;
    rdfs:subClassOf risk-owl:ServiceRelatedConsequence ;
    sw:term_status "accepted"@en ;
    skos:definition "Concept representing limitation of legal support"@en ;
    skos:prefLabel "Legal Support Limited"@en .

risk-owl:LegallyRelevantConsequence a rdfs:Class,
        owl:Class,
        dpv-owl:RiskConcept,
        risk-owl:PotentialConsequence,
        risk-owl:PotentialImpact,
        risk-owl:PotentialRisk ;
    dct:created "2024-12-17"^^xsd:date ;
    rdfs:isDefinedBy risk-owl: ;
    rdfs:subClassOf risk-owl:LegalRiskConcept ;
    sw:term_status "accepted"@en ;
    skos:definition "A consequence that is legally relevant i.e. actionable under law"@en ;
    skos:prefLabel "Legally Relevant Consequence"@en .

risk-owl:LoggingControl a rdfs:Class,
        owl:Class,
        risk-owl:RiskControl ;
    dct:contributor _:N9c63c24625fe482386a350b4ea27b4f8,
        _:Ne22a67b17c7e4a779c30d2864b6a0cee ;
    dct:created "2025-01-06"^^xsd:date ;
    rdfs:isDefinedBy risk-owl: ;
    rdfs:subClassOf risk-owl:MonitorControl ;
    sw:term_status "accepted"@en ;
    skos:definition "Control that logs an event"@en ;
    skos:prefLabel "Logging Control"@en ;
    skos:scopeNote "Log refers to a record of information regarding the event, including whether it has occured, was prevented from occuring, and any actions or processes taken in response to it or resulting from it"@en .

risk-owl:LoseCredibility a rdfs:Class,
        owl:Class,
        dpv-owl:RiskConcept,
        risk-owl:PotentialConsequence,
        risk-owl:PotentialImpact,
        risk-owl:PotentialRisk ;
    dct:contributor _:Ne22a67b17c7e4a779c30d2864b6a0cee ;
    dct:created "2022-08-17"^^xsd:date ;
    dct:modified "2024-08-16"^^xsd:date ;
    dct:source [ a schema:WebPage ;
            schema:name "ISO/IEC 27005:2018" ;
            schema:url "https://www.iso.org/standard/75281.html" ] ;
    rdfs:isDefinedBy risk-owl: ;
    rdfs:subClassOf risk-owl:ReputationalRisk ;
    sw:term_status "accepted"@en ;
    skos:definition "Concept representing Loss of Credibility"@en ;
    skos:prefLabel "Lose of Credibility"@en .

risk-owl:LoseCustomerConfidence a rdfs:Class,
        owl:Class,
        dpv-owl:RiskConcept,
        risk-owl:PotentialConsequence,
        risk-owl:PotentialImpact,
        risk-owl:PotentialRisk ;
    dct:contributor _:Ne22a67b17c7e4a779c30d2864b6a0cee ;
    dct:created "2022-08-17"^^xsd:date ;
    dct:modified "2024-08-16"^^xsd:date ;
    dct:source [ a schema:WebPage ;
            schema:name "ISO/IEC 27005:2018" ;
            schema:url "https://www.iso.org/standard/75281.html" ] ;
    rdfs:isDefinedBy risk-owl: ;
    rdfs:subClassOf risk-owl:ReputationalRisk ;
    sw:term_status "accepted"@en ;
    skos:definition "Concept representing Loss of Customer Confidence"@en ;
    skos:prefLabel "Lose of Customer Confidence"@en .

risk-owl:LoseGoodwill a rdfs:Class,
        owl:Class,
        dpv-owl:RiskConcept,
        risk-owl:PotentialConsequence,
        risk-owl:PotentialImpact,
        risk-owl:PotentialRisk ;
    dct:contributor _:Ne22a67b17c7e4a779c30d2864b6a0cee ;
    dct:created "2022-08-17"^^xsd:date ;
    dct:modified "2024-08-16"^^xsd:date ;
    dct:source [ a schema:WebPage ;
            schema:name "ISO/IEC 27005:2018" ;
            schema:url "https://www.iso.org/standard/75281.html" ] ;
    rdfs:isDefinedBy risk-owl: ;
    rdfs:subClassOf risk-owl:ReputationalRisk ;
    sw:term_status "accepted"@en ;
    skos:definition "Concept representing Loss of Goodwill"@en ;
    skos:prefLabel "Lose of Goodwill"@en .

risk-owl:LoseNegotiatingCapacity a rdfs:Class,
        owl:Class,
        dpv-owl:RiskConcept,
        risk-owl:PotentialConsequence,
        risk-owl:PotentialImpact,
        risk-owl:PotentialRisk ;
    dct:contributor _:Ne22a67b17c7e4a779c30d2864b6a0cee ;
    dct:created "2022-08-17"^^xsd:date ;
    dct:modified "2024-08-16"^^xsd:date ;
    dct:source [ a schema:WebPage ;
            schema:name "ISO/IEC 27005:2018" ;
            schema:url "https://www.iso.org/standard/75281.html" ] ;
    rdfs:isDefinedBy risk-owl: ;
    rdfs:subClassOf risk-owl:ReputationalRisk ;
    sw:term_status "accepted"@en ;
    skos:definition "Concept representing Loss of Negotiating Capacity"@en ;
    skos:prefLabel "Lose of Negotiating Capacity"@en .

risk-owl:LoseOpportunity a rdfs:Class,
        owl:Class,
        dpv-owl:RiskConcept,
        risk-owl:PotentialConsequence,
        risk-owl:PotentialImpact,
        risk-owl:PotentialRisk ;
    dct:contributor _:Ne22a67b17c7e4a779c30d2864b6a0cee ;
    dct:created "2022-08-17"^^xsd:date ;
    dct:modified "2024-08-16"^^xsd:date ;
    dct:source [ a schema:WebPage ;
            schema:name "ISO/IEC 27005:2018" ;
            schema:url "https://www.iso.org/standard/75281.html" ] ;
    rdfs:isDefinedBy risk-owl: ;
    rdfs:subClassOf risk-owl:ReputationalRisk ;
    sw:term_status "accepted"@en ;
    skos:definition "Concept representing Loss of Opportunity"@en ;
    skos:prefLabel "Lose of Opportunity"@en .

risk-owl:LoseReputation a rdfs:Class,
        owl:Class,
        dpv-owl:RiskConcept,
        risk-owl:PotentialConsequence,
        risk-owl:PotentialImpact,
        risk-owl:PotentialRisk ;
    dct:contributor _:Ne22a67b17c7e4a779c30d2864b6a0cee ;
    dct:created "2022-08-17"^^xsd:date ;
    dct:modified "2024-08-16"^^xsd:date ;
    dct:source [ a schema:WebPage ;
            schema:name "ISO/IEC 27005:2018" ;
            schema:url "https://www.iso.org/standard/75281.html" ] ;
    rdfs:isDefinedBy risk-owl: ;
    rdfs:subClassOf risk-owl:ReputationalRisk ;
    sw:term_status "accepted"@en ;
    skos:definition "Concept representing Loss of Reputation"@en ;
    skos:prefLabel "Lose of Reputation"@en .

risk-owl:LoseTrust a rdfs:Class,
        owl:Class,
        dpv-owl:RiskConcept,
        risk-owl:PotentialConsequence,
        risk-owl:PotentialImpact,
        risk-owl:PotentialRisk ;
    dct:contributor _:Ne22a67b17c7e4a779c30d2864b6a0cee ;
    dct:created "2022-08-17"^^xsd:date ;
    dct:modified "2024-08-16"^^xsd:date ;
    dct:source [ a schema:WebPage ;
            schema:name "ISO/IEC 27005:2018" ;
            schema:url "https://www.iso.org/standard/75281.html" ] ;
    rdfs:isDefinedBy risk-owl: ;
    rdfs:subClassOf risk-owl:ReputationalRisk ;
    sw:term_status "accepted"@en ;
    skos:definition "Concept representing Loss of Trust"@en ;
    skos:prefLabel "Lose of Trust"@en .

risk-owl:LowLikelihood a rdfs:Class,
        owl:Class,
        dpv-owl:Likelihood ;
    dct:contributor _:Ne22a67b17c7e4a779c30d2864b6a0cee ;
    dct:created "2022-08-18"^^xsd:date ;
    rdf:value "0.25,xsd:decimal" ;
    rdfs:isDefinedBy risk-owl: ;
    rdfs:subClassOf risk-owl:3LikelihoodLevels,
        risk-owl:5LikelihoodLevels,
        risk-owl:7LikelihoodLevels ;
    sw:term_status "accepted"@en ;
    skos:definition "Level where Likelihood is Low"@en ;
    skos:prefLabel "Low Likelihood"@en ;
    skos:scopeNote "The suggested quantitative value for this concept is 0.25 on a scale of 0 to 1"@en .

risk-owl:LowRisk a rdfs:Class,
        owl:Class,
        dpv-owl:RiskLevel ;
    dct:contributor _:Ne22a67b17c7e4a779c30d2864b6a0cee ;
    dct:created "2022-08-18"^^xsd:date ;
    rdf:value "0.25,xsd:decimal" ;
    rdfs:isDefinedBy risk-owl: ;
    rdfs:subClassOf risk-owl:3RiskLevels,
        risk-owl:5RiskLevels,
        risk-owl:7RiskLevels ;
    sw:term_status "accepted"@en ;
    skos:definition "Level where Risk is Low"@en ;
    skos:prefLabel "Low Risk"@en ;
    skos:scopeNote "The suggested quantitative value for this concept is 0.25 on a scale of 0 to 1"@en .

risk-owl:LowSeverity a rdfs:Class,
        owl:Class,
        dpv-owl:Severity ;
    dct:contributor _:Ne22a67b17c7e4a779c30d2864b6a0cee ;
    dct:created "2022-08-18"^^xsd:date ;
    rdf:value "0.25,xsd:decimal" ;
    rdfs:isDefinedBy risk-owl: ;
    rdfs:subClassOf risk-owl:3SeverityLevels,
        risk-owl:5SeverityLevels,
        risk-owl:7SeverityLevels ;
    sw:term_status "accepted"@en ;
    skos:definition "Level where Severity is Low"@en ;
    skos:prefLabel "Low Severity"@en ;
    skos:scopeNote "The suggested quantitative value for this concept is 0.25 on a scale of 0 to 1"@en .

risk-owl:LoyaltyProgramExclusion a rdfs:Class,
        owl:Class,
        dpv-owl:RiskConcept,
        risk-owl:PotentialConsequence,
        risk-owl:PotentialImpact,
        risk-owl:PotentialRisk ;
    dct:created "2024-10-21"^^xsd:date ;
    rdfs:isDefinedBy risk-owl: ;
    rdfs:subClassOf risk-owl:ServiceRelatedConsequence ;
    sw:term_status "accepted"@en ;
    skos:definition "Concept representing exclusion from loyalty program"@en ;
    skos:prefLabel "Loyalty Program Exclusion"@en .

risk-owl:MaliciousActivity a rdfs:Class,
        owl:Class,
        dpv-owl:RiskConcept,
        risk-owl:PotentialConsequence,
        risk-owl:PotentialRisk,
        risk-owl:PotentialRiskSource ;
    dct:created "2024-12-17"^^xsd:date ;
    rdfs:isDefinedBy risk-owl: ;
    rdfs:subClassOf risk-owl:ExternalSecurityThreat ;
    sw:term_status "accepted"@en ;
    skos:definition "Intentional actions designed to harm, exploit, manipulate, or disrupt individuals, systems, or organizations for personal gain or detriment to others"@en ;
    skos:prefLabel "Malicious Activity"@en .

risk-owl:MaliciousCodeAttack a rdfs:Class,
        owl:Class,
        dpv-owl:RiskConcept,
        risk-owl:AvailabilityConcept,
        risk-owl:ConfidentialityConcept,
        risk-owl:IntegrityConcept,
        risk-owl:PotentialRisk,
        risk-owl:PotentialRiskSource ;
    dct:contributor _:Ne22a67b17c7e4a779c30d2864b6a0cee ;
    dct:created "2022-08-17"^^xsd:date ;
    dct:modified "2024-08-16"^^xsd:date ;
    dct:source [ a schema:WebPage ;
            schema:name "ENISA Reference Incident Classification Taxonomy 2018" ;
            schema:url "https://www.enisa.europa.eu/publications/reference-incident-classification-taxonomy/" ] ;
    rdfs:isDefinedBy risk-owl: ;
    rdfs:subClassOf risk-owl:SecurityAttack ;
    sw:term_status "accepted"@en ;
    skos:definition "Concept representing Malicious Code Attack"@en ;
    skos:prefLabel "Malicious Code Attack"@en .

risk-owl:MalwareAttack a rdfs:Class,
        owl:Class,
        dpv-owl:RiskConcept,
        risk-owl:AvailabilityConcept,
        risk-owl:ConfidentialityConcept,
        risk-owl:IntegrityConcept,
        risk-owl:PotentialRisk,
        risk-owl:PotentialRiskSource ;
    dct:contributor _:Ne22a67b17c7e4a779c30d2864b6a0cee ;
    dct:created "2022-08-17"^^xsd:date ;
    dct:modified "2024-08-16"^^xsd:date ;
    dct:source [ a schema:WebPage ;
            schema:name "ENISA Methodology for Sectoral Cybersecurity Assessments" ;
            schema:url "https://www.enisa.europa.eu/publications/methodology-for-a-sectoral-cybersecurity-assessment" ] ;
    rdfs:isDefinedBy risk-owl: ;
    rdfs:subClassOf risk-owl:SecurityAttack ;
    sw:term_status "accepted"@en ;
    skos:definition "Concept representing Malware Attack"@en ;
    skos:prefLabel "Malware Attack"@en .

risk-owl:MaterialDamage a rdfs:Class,
        owl:Class,
        dpv-owl:RiskConcept,
        risk-owl:PotentialConsequence,
        risk-owl:PotentialImpact,
        risk-owl:PotentialRisk ;
    dct:contributor _:Ne22a67b17c7e4a779c30d2864b6a0cee ;
    dct:created "2022-03-30"^^xsd:date ;
    dct:modified "2024-08-16"^^xsd:date ;
    rdfs:isDefinedBy risk-owl: ;
    rdfs:subClassOf risk-owl:LegallyRelevantConsequence ;
    sw:term_status "accepted"@en ;
    skos:definition "Concept representing Material Damage"@en ;
    skos:prefLabel "Material Damage"@en ;
    skos:scopeNote "The criteria for what is considered material damage is based in jurisdictional laws and norms"@en .

risk-owl:MentalHealth a rdfs:Class,
        owl:Class,
        dpv-owl:RiskConcept,
        risk-owl:PotentialConsequence,
        risk-owl:PotentialImpact,
        risk-owl:PotentialRisk ;
    dct:contributor _:Ne22a67b17c7e4a779c30d2864b6a0cee ;
    dct:created "2024-12-01"^^xsd:date ;
    rdfs:isDefinedBy risk-owl: ;
    rdfs:subClassOf risk-owl:Health ;
    sw:term_status "accepted"@en ;
    skos:definition "Concept representing mental health of individual(s), or group(s), or society at large"@en ;
    skos:prefLabel "Mental Health"@en .

risk-owl:MentalSafety a rdfs:Class,
        owl:Class,
        dpv-owl:RiskConcept,
        risk-owl:PotentialConsequence,
        risk-owl:PotentialImpact,
        risk-owl:PotentialRisk ;
    dct:contributor _:Ne22a67b17c7e4a779c30d2864b6a0cee ;
    dct:created "2024-12-01"^^xsd:date ;
    rdfs:isDefinedBy risk-owl: ;
    rdfs:subClassOf risk-owl:Safety ;
    sw:term_status "accepted"@en ;
    skos:definition "Concept representing mental safety of individual(s), or group(s), or society at large"@en ;
    skos:prefLabel "Mental Safety"@en .

risk-owl:Misandry a rdfs:Class,
        owl:Class,
        dpv-owl:RiskConcept,
        risk-owl:PotentialConsequence,
        risk-owl:PotentialImpact,
        risk-owl:PotentialRisk ;
    dct:created "2024-09-30"^^xsd:date ;
    rdfs:isDefinedBy risk-owl: ;
    rdfs:subClassOf risk-owl:Sexism ;
    sw:term_status "accepted"@en ;
    skos:definition "Dislike, contempt, or prejudice against men"@en ;
    skos:prefLabel "Misandry"@en .

risk-owl:Misogyny a rdfs:Class,
        owl:Class,
        dpv-owl:RiskConcept,
        risk-owl:PotentialConsequence,
        risk-owl:PotentialImpact,
        risk-owl:PotentialRisk ;
    dct:created "2024-09-30"^^xsd:date ;
    rdfs:isDefinedBy risk-owl: ;
    rdfs:subClassOf risk-owl:Sexism ;
    sw:term_status "accepted"@en ;
    skos:definition "Dislike, contempt, or prejudice against women"@en ;
    skos:prefLabel "Misogyny"@en .

risk-owl:Misuse a rdfs:Class,
        owl:Class,
        dpv-owl:RiskConcept,
        risk-owl:PotentialConsequence,
        risk-owl:PotentialRisk,
        risk-owl:PotentialRiskSource ;
    dct:contributor _:N9c63c24625fe482386a350b4ea27b4f8 ;
    dct:created "2024-06-11"^^xsd:date ;
    dct:modified "2024-08-16"^^xsd:date ;
    rdfs:isDefinedBy risk-owl: ;
    rdfs:subClassOf risk-owl:UserRisks ;
    sw:term_status "accepted"@en ;
    skos:definition "Concept representing a misuse (of something)"@en ;
    skos:prefLabel "Misuse"@en .

risk-owl:MitigationControl a rdfs:Class,
        owl:Class,
        risk-owl:RiskControl ;
    dct:contributor _:N9c63c24625fe482386a350b4ea27b4f8,
        _:Ne22a67b17c7e4a779c30d2864b6a0cee ;
    dct:created "2025-01-06"^^xsd:date ;
    rdfs:isDefinedBy risk-owl: ;
    rdfs:subClassOf risk-owl:ProactiveControl ;
    sw:term_status "accepted"@en ;
    skos:definition "Control that aims to reduce the likelihood or effect of an event with the goal of managing an event accepted to occur"@en ;
    skos:prefLabel "Mitigation Control"@en ;
    skos:scopeNote "Mitigation requires accepting that an event will occur, and thereby focusing on managing it by reducing its likelihood or effects by adding additional processes to specifically address the event or its effects"@en .

risk-owl:ModerateLikelihood a rdfs:Class,
        owl:Class,
        dpv-owl:Likelihood ;
    dct:contributor _:Ne22a67b17c7e4a779c30d2864b6a0cee ;
    dct:created "2022-08-18"^^xsd:date ;
    rdf:value "0.5,xsd:decimal" ;
    rdfs:isDefinedBy risk-owl: ;
    rdfs:subClassOf risk-owl:3LikelihoodLevels,
        risk-owl:5LikelihoodLevels,
        risk-owl:7LikelihoodLevels ;
    sw:term_status "accepted"@en ;
    skos:definition "Level where Likelihood is Moderate"@en ;
    skos:prefLabel "Moderate Likelihood"@en ;
    skos:scopeNote "The suggested quantitative value for this concept is 0.5 on a scale of 0 to 1"@en .

risk-owl:ModerateRisk a rdfs:Class,
        owl:Class,
        dpv-owl:RiskLevel ;
    dct:contributor _:Ne22a67b17c7e4a779c30d2864b6a0cee ;
    dct:created "2022-08-18"^^xsd:date ;
    rdf:value "0.5,xsd:decimal" ;
    rdfs:isDefinedBy risk-owl: ;
    rdfs:subClassOf risk-owl:3RiskLevels,
        risk-owl:5RiskLevels,
        risk-owl:7RiskLevels ;
    sw:term_status "accepted"@en ;
    skos:definition "Level where Risk is Moderate"@en ;
    skos:prefLabel "Moderate Risk"@en ;
    skos:scopeNote "The suggested quantitative value for this concept is 0.5 on a scale of 0 to 1"@en .

risk-owl:ModerateSeverity a rdfs:Class,
        owl:Class,
        dpv-owl:Severity ;
    dct:contributor _:Ne22a67b17c7e4a779c30d2864b6a0cee ;
    dct:created "2022-08-18"^^xsd:date ;
    rdf:value "0.5,xsd:decimal" ;
    rdfs:isDefinedBy risk-owl: ;
    rdfs:subClassOf risk-owl:3SeverityLevels,
        risk-owl:5SeverityLevels,
        risk-owl:7SeverityLevels ;
    sw:term_status "accepted"@en ;
    skos:definition "Level where Severity is Moderate"@en ;
    skos:prefLabel "Moderate Severity"@en ;
    skos:scopeNote "The suggested quantitative value for this concept is 0.5 on a scale of 0 to 1"@en .

risk-owl:ModificationControl a rdfs:Class,
        owl:Class,
        risk-owl:RiskControl ;
    dct:contributor _:N9c63c24625fe482386a350b4ea27b4f8,
        _:Ne22a67b17c7e4a779c30d2864b6a0cee ;
    dct:created "2025-01-06"^^xsd:date ;
    rdfs:isDefinedBy risk-owl: ;
    rdfs:subClassOf risk-owl:ProactiveControl ;
    sw:term_status "accepted"@en ;
    skos:definition "Control that modifies the context to change the event's characteristics such that the event still occurs but with the modified characteristics with the goal of managing an event that is accepted to occur"@en ;
    skos:prefLabel "Modification Control"@en ;
    skos:scopeNote "Modification necessitates a change in the context to result in a change in the event's characteristics. Where such changes reduce the likelihood or effects of the event, the modification also works as a mitigation for the event"@en .

risk-owl:MonitorConsequence a rdfs:Class,
        owl:Class,
        risk-owl:RiskControl ;
    dct:contributor _:Ne22a67b17c7e4a779c30d2864b6a0cee ;
    dct:created "2024-05-19"^^xsd:date ;
    dct:modified "2025-01-06"^^xsd:date ;
    rdfs:isDefinedBy risk-owl: ;
    rdfs:subClassOf risk-owl:MonitorControl ;
    sw:term_status "modified"@en ;
    skos:definition "Control that monitors a Risk Consequence"@en ;
    skos:prefLabel "Monitor Consequence"@en .

risk-owl:MonitorControl a rdfs:Class,
        owl:Class,
        risk-owl:RiskControl ;
    dct:contributor _:Ne22a67b17c7e4a779c30d2864b6a0cee ;
    dct:created "2024-05-19"^^xsd:date ;
    dct:modified "2025-01-06"^^xsd:date ;
    rdfs:isDefinedBy risk-owl: ;
    rdfs:subClassOf risk-owl:ProactiveControl ;
    sw:term_status "modified"@en ;
    skos:definition "Control that monitors for the occurence of an event"@en ;
    skos:prefLabel "Monitor Control"@en ;
    skos:scopeNote "Monitoring is a broad term that refers to identifying information about an event, including its occurence, characteristics such as severity or specific contextual metrics, affected things and entities, and having the ability to obtain and use this information to address the event. Monitoring is also used to refer to the activities associated with ensuring controls are active and effective. For this reason, specific concepts are defined which extend this control to express explicit actions included in the general use of 'monitoring' in risk management"@en .

risk-owl:MonitorImpact a rdfs:Class,
        owl:Class,
        risk-owl:RiskControl ;
    dct:contributor _:Ne22a67b17c7e4a779c30d2864b6a0cee ;
    dct:created "2024-05-19"^^xsd:date ;
    dct:modified "2025-01-06"^^xsd:date ;
    rdfs:isDefinedBy risk-owl: ;
    rdfs:subClassOf risk-owl:MonitorControl ;
    sw:term_status "modified"@en ;
    skos:definition "Control that monitors a Risk Impact"@en ;
    skos:prefLabel "Monitor Impact"@en .

risk-owl:MonitorRisk a rdfs:Class,
        owl:Class,
        risk-owl:RiskControl ;
    dct:contributor _:Ne22a67b17c7e4a779c30d2864b6a0cee ;
    dct:created "2024-05-19"^^xsd:date ;
    dct:modified "2025-01-06"^^xsd:date ;
    rdfs:isDefinedBy risk-owl: ;
    rdfs:subClassOf risk-owl:MonitorControl ;
    sw:term_status "modified"@en ;
    skos:definition "Control that monitors a Risk"@en ;
    skos:prefLabel "Monitor Risk"@en .

risk-owl:MonitorRiskControl a rdfs:Class,
        owl:Class,
        risk-owl:RiskControl ;
    dct:contributor _:Ne22a67b17c7e4a779c30d2864b6a0cee ;
    dct:created "2024-05-19"^^xsd:date ;
    dct:modified "2025-01-06"^^xsd:date ;
    rdfs:isDefinedBy risk-owl: ;
    rdfs:subClassOf risk-owl:MonitorControl ;
    sw:term_status "modified"@en ;
    skos:definition "Control that monitors another Control"@en ;
    skos:prefLabel "Monitor Control"@en .

risk-owl:MonitorRiskSource a rdfs:Class,
        owl:Class,
        risk-owl:RiskControl ;
    dct:contributor _:Ne22a67b17c7e4a779c30d2864b6a0cee ;
    dct:created "2024-05-19"^^xsd:date ;
    dct:modified "2025-01-06"^^xsd:date ;
    rdfs:isDefinedBy risk-owl: ;
    rdfs:subClassOf risk-owl:MonitorControl ;
    sw:term_status "modified"@en ;
    skos:definition "Control that monitors a Risk Source"@en ;
    skos:prefLabel "Monitor Risk Source"@en .

risk-owl:MonitorVulnerabilities a rdfs:Class,
        owl:Class,
        risk-owl:RiskControl ;
    dct:contributor _:Ne22a67b17c7e4a779c30d2864b6a0cee ;
    dct:created "2024-05-19"^^xsd:date ;
    dct:modified "2025-01-06"^^xsd:date ;
    rdfs:isDefinedBy risk-owl: ;
    rdfs:subClassOf risk-owl:MonitorControl ;
    sw:term_status "modified"@en ;
    skos:definition "Control that monitors a Risk Vulnerability"@en ;
    skos:prefLabel "Monitor Vulnerabilities"@en .

risk-owl:NationalityDiscrimination a rdfs:Class,
        owl:Class,
        dpv-owl:RiskConcept,
        risk-owl:PotentialConsequence,
        risk-owl:PotentialImpact,
        risk-owl:PotentialRisk ;
    dct:created "2024-09-30"^^xsd:date ;
    rdfs:isDefinedBy risk-owl: ;
    rdfs:subClassOf risk-owl:Discrimination ;
    sw:term_status "accepted"@en ;
    skos:definition "Discrimination based on a person's nationality or citizenship"@en ;
    skos:prefLabel "Nationality Discrimination"@en .

risk-owl:NonMaterialDamage a rdfs:Class,
        owl:Class,
        dpv-owl:RiskConcept,
        risk-owl:PotentialConsequence,
        risk-owl:PotentialImpact,
        risk-owl:PotentialRisk ;
    dct:contributor _:Ne22a67b17c7e4a779c30d2864b6a0cee ;
    dct:created "2022-03-30"^^xsd:date ;
    dct:modified "2024-08-16"^^xsd:date ;
    rdfs:isDefinedBy risk-owl: ;
    rdfs:subClassOf risk-owl:LegallyRelevantConsequence ;
    sw:term_status "accepted"@en ;
    skos:definition "Concept representing Non-Material Damage"@en ;
    skos:prefLabel "Non-Material Damage"@en ;
    skos:scopeNote "The criteria for what is considered material damage is based in jurisdictional laws and norms"@en .

risk-owl:NonNormalityBias a rdfs:Class,
        owl:Class,
        dpv-owl:RiskConcept,
        risk-owl:PotentialConsequence,
        risk-owl:PotentialRisk,
        risk-owl:PotentialRiskSource ;
    dct:contributor _:N2e9307242cb14d528effb994db501842,
        _:N9c63c24625fe482386a350b4ea27b4f8,
        _:Ne22a67b17c7e4a779c30d2864b6a0cee ;
    dct:created "2024-09-13"^^xsd:date ;
    dct:source "ISO/IEC 24027:2021"@en ;
    rdfs:isDefinedBy risk-owl: ;
    rdfs:subClassOf risk-owl:StatisticalBias ;
    sw:term_status "accepted"@en ;
    skos:definition "Bias that occurs when the dataset is subject to a different (i.e. non-normal) distribution (e.g., Chi-Square, Beta, Lorentz, Cauchy, Weibull or Pareto) where the results can be biased and misleading"@en ;
    skos:prefLabel "Non-Normality Bias"@en .

risk-owl:NonResponseBias a rdfs:Class,
        owl:Class,
        dpv-owl:RiskConcept,
        risk-owl:PotentialConsequence,
        risk-owl:PotentialRisk,
        risk-owl:PotentialRiskSource ;
    dct:contributor _:N2e9307242cb14d528effb994db501842,
        _:N9c63c24625fe482386a350b4ea27b4f8,
        _:Ne22a67b17c7e4a779c30d2864b6a0cee ;
    dct:created "2024-09-13"^^xsd:date ;
    dct:source "ISO/IEC 24027:2021"@en ;
    rdfs:isDefinedBy risk-owl: ;
    rdfs:subClassOf risk-owl:SelectionBias ;
    sw:term_status "accepted"@en ;
    skos:definition "Bias that occurs when people from certain groups opt-out of surveys at different rates than users from other groups. This is also called as Participation bias"@en ;
    skos:prefLabel "Non-Response Bias"@en .

risk-owl:OperationalSecurityRisk a rdfs:Class,
        owl:Class,
        dpv-owl:RiskConcept,
        risk-owl:PotentialConsequence,
        risk-owl:PotentialRisk,
        risk-owl:PotentialRiskSource ;
    dct:created "2024-12-17"^^xsd:date ;
    rdfs:isDefinedBy risk-owl: ;
    rdfs:subClassOf risk-owl:TechnicalRiskConcept ;
    sw:term_status "accepted"@en ;
    skos:definition "Risks and issues that arise during operational processes"@en ;
    skos:prefLabel "Operational Security Risk"@en .

risk-owl:OrganisationalManagementRisk a rdfs:Class,
        owl:Class,
        dpv-owl:RiskConcept,
        risk-owl:PotentialConsequence,
        risk-owl:PotentialRisk,
        risk-owl:PotentialRiskSource ;
    dct:contributor _:N9c63c24625fe482386a350b4ea27b4f8,
        _:Ne22a67b17c7e4a779c30d2864b6a0cee ;
    dct:created "2024-12-01"^^xsd:date ;
    rdfs:isDefinedBy risk-owl: ;
    rdfs:subClassOf risk-owl:OrganisationalRiskConcept ;
    sw:term_status "accepted"@en ;
    skos:definition "Concept representing issues and risks associated with the management of operations and resources by the organisation"@en ;
    skos:prefLabel "Organisational Management Risk"@en .

risk-owl:OrganisationalRiskConcept a rdfs:Class,
        owl:Class,
        dpv-owl:RiskConcept,
        risk-owl:PotentialConsequence,
        risk-owl:PotentialImpact,
        risk-owl:PotentialRisk,
        risk-owl:PotentialRiskSource ;
    dct:created "2024-10-21"^^xsd:date ;
    rdfs:isDefinedBy risk-owl: ;
    rdfs:subClassOf dpv-owl:RiskConcept ;
    sw:term_status "accepted"@en ;
    skos:definition "Risk concepts, including any potential risk sources, consequences, or impacts, that are organisational in nature or relate to an organisational process"@en ;
    skos:prefLabel "Organisational Risk Concept"@en ;
    skos:scopeNote "Organisational in this context refers to an organisation which is not human but is managed by humans"@en .

risk-owl:OutGroupHomogeneityBias a rdfs:Class,
        owl:Class,
        dpv-owl:RiskConcept,
        risk-owl:PotentialConsequence,
        risk-owl:PotentialRisk,
        risk-owl:PotentialRiskSource ;
    dct:contributor _:N2e9307242cb14d528effb994db501842,
        _:N9c63c24625fe482386a350b4ea27b4f8,
        _:Ne22a67b17c7e4a779c30d2864b6a0cee ;
    dct:created "2024-09-13"^^xsd:date ;
    dct:source "ISO/IEC 24027:2021"@en ;
    rdfs:isDefinedBy risk-owl: ;
    rdfs:subClassOf risk-owl:CognitiveBias ;
    sw:term_status "accepted"@en ;
    skos:definition "Bias that occurs when seeing out-group members as more alike than in-group members when comparing attitudes, values, personality traits, and other characteristics"@en ;
    skos:prefLabel "Out-Group Homogeneity Bias"@en .

risk-owl:OverrideControl a rdfs:Class,
        owl:Class,
        risk-owl:RiskControl ;
    dct:contributor _:N9c63c24625fe482386a350b4ea27b4f8,
        _:Ne22a67b17c7e4a779c30d2864b6a0cee ;
    dct:created "2025-01-06"^^xsd:date ;
    rdfs:isDefinedBy risk-owl: ;
    rdfs:subClassOf risk-owl:ReactiveControl ;
    sw:term_status "accepted"@en ;
    skos:definition "Control that aims to override the event with the goal of avoiding its further effects"@en ;
    skos:prefLabel "Override Control"@en ;
    skos:scopeNote "Override indicates a (temporary) change or bypassing of usual processes, controls, and measures in response to an event"@en .

risk-owl:OversightControl a rdfs:Class,
        owl:Class,
        risk-owl:RiskControl ;
    dct:contributor _:Ne22a67b17c7e4a779c30d2864b6a0cee ;
    dct:created "2025-01-06"^^xsd:date ;
    rdfs:isDefinedBy risk-owl: ;
    rdfs:subClassOf risk-owl:MonitorControl ;
    sw:term_status "accepted"@en ;
    skos:definition "Control that provides oversight for an event in terms of having information about it and being able to supervise or manage it"@en ;
    skos:prefLabel "Oversight Control"@en ;
    skos:scopeNote "Oversight can be ambigiously used in terms of having knowledge about an event (see risk:TransparencyControl instead), or being able to identify when it occurs (see risk:DetectionControl instead). The control defined by this concept includes the ability to act on the event as part of the 'oversight' term used in management"@en .

risk-owl:Payment a rdfs:Class,
        owl:Class,
        dpv-owl:RiskConcept,
        risk-owl:PotentialConsequence,
        risk-owl:PotentialImpact,
        risk-owl:PotentialRisk ;
    dct:contributor _:N7d9b5ee7f31f4f2ba5951e30b49ec7c0,
        _:Ne22a67b17c7e4a779c30d2864b6a0cee ;
    dct:created "2024-04-14"^^xsd:date ;
    dct:modified "2024-08-16"^^xsd:date ;
    rdfs:isDefinedBy risk-owl: ;
    rdfs:subClassOf risk-owl:Renumeration ;
    sw:term_status "accepted"@en ;
    skos:definition "Something that acts as or provides payment e.g. to access a service or purchase resources"@en ;
    skos:prefLabel "Payment"@en .

risk-owl:PersonalSafetyEndangerment a rdfs:Class,
        owl:Class,
        dpv-owl:RiskConcept,
        risk-owl:PotentialConsequence,
        risk-owl:PotentialImpact,
        risk-owl:PotentialRisk ;
    dct:contributor _:Ne22a67b17c7e4a779c30d2864b6a0cee ;
    dct:created "2022-08-17"^^xsd:date ;
    dct:modified "2024-12-01"^^xsd:date ;
    dct:source [ a schema:WebPage ;
            schema:name "ISO/IEC 27005:2018" ;
            schema:url "https://www.iso.org/standard/75281.html" ] ;
    rdfs:isDefinedBy risk-owl: ;
    rdfs:subClassOf risk-owl:IndividualRisk ;
    sw:term_status "modified"@en ;
    skos:definition "Concept representing Personal Safety Endangerment"@en ;
    skos:prefLabel "Personal Safety Endangerment"@en .

risk-owl:PersonalisationDisabled a rdfs:Class,
        owl:Class,
        dpv-owl:RiskConcept,
        risk-owl:PotentialConsequence,
        risk-owl:PotentialImpact,
        risk-owl:PotentialRisk ;
    dct:created "2024-10-21"^^xsd:date ;
    rdfs:isDefinedBy risk-owl: ;
    rdfs:subClassOf risk-owl:ServiceRelatedConsequence ;
    sw:term_status "accepted"@en ;
    skos:definition "Concept representing personalisation disabled"@en ;
    skos:prefLabel "Personalisation Disabled"@en .

risk-owl:PersonalisationEnabled a rdfs:Class,
        owl:Class,
        dpv-owl:RiskConcept,
        risk-owl:PotentialConsequence,
        risk-owl:PotentialImpact,
        risk-owl:PotentialRisk ;
    dct:created "2024-10-21"^^xsd:date ;
    rdfs:isDefinedBy risk-owl: ;
    rdfs:subClassOf risk-owl:ServiceRelatedConsequence ;
    sw:term_status "accepted"@en ;
    skos:definition "Concept representing personalisation enabled"@en ;
    skos:prefLabel "Personalisation Enabled"@en .

risk-owl:PhishingScam a rdfs:Class,
        owl:Class,
        dpv-owl:RiskConcept,
        risk-owl:ConfidentialityConcept,
        risk-owl:PotentialConsequence,
        risk-owl:PotentialRisk,
        risk-owl:PotentialRiskSource ;
    dct:contributor _:Ne22a67b17c7e4a779c30d2864b6a0cee ;
    dct:created "2022-08-17"^^xsd:date ;
    dct:modified "2024-08-16"^^xsd:date ;
    dct:source [ a schema:WebPage ;
            schema:name "ENISA Threat Landscape for Ransomware Attacks 2022" ;
            schema:url "https://www.enisa.europa.eu/publications/enisa-threat-landscape-for-ransomware-attacks" ] ;
    rdfs:isDefinedBy risk-owl: ;
    rdfs:subClassOf risk-owl:MaliciousActivity ;
    sw:term_status "accepted"@en ;
    skos:definition "Concept representing Phishing Scam"@en ;
    skos:prefLabel "Phishing Scam"@en .

risk-owl:PhysicalAssault a rdfs:Class,
        owl:Class,
        dpv-owl:RiskConcept,
        risk-owl:PotentialConsequence,
        risk-owl:PotentialImpact,
        risk-owl:PotentialRisk ;
    dct:contributor _:Ne22a67b17c7e4a779c30d2864b6a0cee ;
    dct:created "2022-08-17"^^xsd:date ;
    dct:modified "2024-08-16"^^xsd:date ;
    dct:source [ a schema:WebPage ;
            schema:name "ISO/IEC 27005:2018" ;
            schema:url "https://www.iso.org/standard/75281.html" ] ;
    rdfs:isDefinedBy risk-owl: ;
    rdfs:subClassOf risk-owl:Harm,
        risk-owl:PhysicalSafety ;
    sw:term_status "accepted"@en ;
    skos:definition "Concept representing Physical Assault"@en ;
    skos:prefLabel "Physical Assault"@en .

risk-owl:PhysicalHarm a rdfs:Class,
        owl:Class,
        dpv-owl:RiskConcept,
        risk-owl:PotentialConsequence,
        risk-owl:PotentialImpact,
        risk-owl:PotentialRisk ;
    dct:contributor _:N9c63c24625fe482386a350b4ea27b4f8,
        _:Ne22a67b17c7e4a779c30d2864b6a0cee ;
    dct:created "2022-08-17"^^xsd:date ;
    dct:modified "2024-12-01"^^xsd:date ;
    rdfs:isDefinedBy risk-owl: ;
    rdfs:subClassOf risk-owl:Harm,
        risk-owl:PhysicalHealth ;
    sw:term_status "modified"@en ;
    skos:definition "Concept representing physical harm to an individual or individual(s)"@en ;
    skos:prefLabel "Physical Harm"@en .

risk-owl:PhysicalHealth a rdfs:Class,
        owl:Class,
        dpv-owl:RiskConcept,
        risk-owl:PotentialConsequence,
        risk-owl:PotentialImpact,
        risk-owl:PotentialRisk ;
    dct:contributor _:Ne22a67b17c7e4a779c30d2864b6a0cee ;
    dct:created "2024-12-01"^^xsd:date ;
    rdfs:isDefinedBy risk-owl: ;
    rdfs:subClassOf risk-owl:Health ;
    sw:term_status "accepted"@en ;
    skos:definition "Concept representing physical health of individual(s), or group(s), or society at large"@en ;
    skos:prefLabel "Physical Health"@en .

risk-owl:PhysicalSafety a rdfs:Class,
        owl:Class,
        dpv-owl:RiskConcept,
        risk-owl:PotentialConsequence,
        risk-owl:PotentialImpact,
        risk-owl:PotentialRisk ;
    dct:contributor _:Ne22a67b17c7e4a779c30d2864b6a0cee ;
    dct:created "2024-12-01"^^xsd:date ;
    rdfs:isDefinedBy risk-owl: ;
    rdfs:subClassOf risk-owl:Safety ;
    sw:term_status "accepted"@en ;
    skos:definition "Concept representing physical safety of individual(s), or group(s), or society at large"@en ;
    skos:prefLabel "Physical Safety"@en .

risk-owl:PolicyRisk a rdfs:Class,
        owl:Class,
        dpv-owl:RiskConcept,
        risk-owl:PotentialConsequence,
        risk-owl:PotentialRisk,
        risk-owl:PotentialRiskSource ;
    dct:created "2024-12-17"^^xsd:date ;
    rdfs:isDefinedBy risk-owl: ;
    rdfs:subClassOf risk-owl:LegalRiskConcept ;
    sw:term_status "accepted"@en ;
    skos:definition "Risks and consequences regarding policy and its associated processes"@en ;
    skos:prefLabel "Policy Risk"@en .

risk-owl:PotentialConsequence a rdfs:Class,
        owl:Class ;
    dct:contributor _:Ne22a67b17c7e4a779c30d2864b6a0cee ;
    dct:created "2024-09-29"^^xsd:date ;
    vann:example dex-owl:E0087 ;
    rdfs:isDefinedBy risk-owl: ;
    rdfs:subClassOf dpv-owl:RiskConcept ;
    sw:term_status "accepted"@en ;
    skos:definition "Indicates a concept can potentially be a 'consequence concept within an use-case"@en ;
    skos:prefLabel "Potential Consequence"@en ;
    skos:scopeNote "PotentialConsequence is a suggestion that the concept can be a 'risk' within an use-case - this suggestion is not exclusive and the concept may also be instances of other potential concepts to indicate the multiple possible roles a concept can take. This suggestion can be ignored if it is not applicable to the use-case"@en .

risk-owl:PotentialImpact a rdfs:Class,
        owl:Class ;
    dct:contributor _:Ne22a67b17c7e4a779c30d2864b6a0cee ;
    dct:created "2024-09-29"^^xsd:date ;
    vann:example dex-owl:E0087 ;
    rdfs:isDefinedBy risk-owl: ;
    rdfs:subClassOf dpv-owl:RiskConcept ;
    sw:term_status "accepted"@en ;
    skos:definition "Indicates a concept can potentially be a 'impact' concept within an use-case"@en ;
    skos:prefLabel "Potential Impact"@en ;
    skos:scopeNote "PotentialImpact is a suggestion that the concept can be a 'risk' within an use-case - this suggestion is not exclusive and the concept may also be instances of other potential concepts to indicate the multiple possible roles a concept can take. This suggestion can be ignored if it is not applicable to the use-case"@en .

risk-owl:PotentialRisk a rdfs:Class,
        owl:Class ;
    dct:contributor _:Ne22a67b17c7e4a779c30d2864b6a0cee ;
    dct:created "2024-09-29"^^xsd:date ;
    vann:example dex-owl:E0087 ;
    rdfs:isDefinedBy risk-owl: ;
    rdfs:subClassOf dpv-owl:RiskConcept ;
    sw:term_status "accepted"@en ;
    skos:definition "Indicates a concept can potentially be a 'risk' concept within an use-case"@en ;
    skos:prefLabel "Potential Risk"@en ;
    skos:scopeNote "PotentialRisk is a suggestion that the concept can be a 'risk' within an use-case - this suggestion is not exclusive and the concept may also be instances of other potential concepts to indicate the multiple possible roles a concept can take. This suggestion can be ignored if it is not applicable to the use-case"@en .

risk-owl:PotentialRiskSource a rdfs:Class,
        owl:Class ;
    dct:contributor _:Ne22a67b17c7e4a779c30d2864b6a0cee ;
    dct:created "2024-09-29"^^xsd:date ;
    vann:example dex-owl:E0087 ;
    rdfs:isDefinedBy risk-owl: ;
    rdfs:subClassOf dpv-owl:RiskConcept ;
    sw:term_status "accepted"@en ;
    skos:definition "Indicates a concept can potentially be a 'risk source' concept within an use-case"@en ;
    skos:prefLabel "Potential RiskSource"@en ;
    skos:scopeNote "PotentialRiskSource is a suggestion that the concept can be a 'risk' within an use-case - this suggestion is not exclusive and the concept may also be instances of other potential concepts to indicate the multiple possible roles a concept can take. This suggestion can be ignored if it is not applicable to the use-case"@en .

risk-owl:Privacy a rdfs:Class,
        owl:Class,
        dpv-owl:RiskConcept,
        risk-owl:PotentialConsequence,
        risk-owl:PotentialImpact,
        risk-owl:PotentialRisk ;
    dct:created "2024-12-17"^^xsd:date ;
    rdfs:isDefinedBy risk-owl: ;
    rdfs:subClassOf risk-owl:IndividualRisk ;
    sw:term_status "accepted"@en ;
    skos:definition "Concept representing privacy of humans at an individual, group, or larger societal levels"@en ;
    skos:prefLabel "Privacy"@en .

risk-owl:ProactiveControl a rdfs:Class,
        owl:Class,
        risk-owl:RiskControl ;
    dct:contributor _:Ne22a67b17c7e4a779c30d2864b6a0cee ;
    dct:created "2025-01-06"^^xsd:date ;
    rdfs:isDefinedBy risk-owl: ;
    rdfs:subClassOf risk-owl:RiskControl ;
    sw:term_status "accepted"@en ;
    skos:definition "Control that is established or functions before an event occurs"@en ;
    skos:prefLabel "Proactive Control"@en ;
    skos:scopeNote "The use of 'proactive' here refers to this control being established to address events before they occur. It does not indicate putting in place controls before the event such as planning ahead for potential use of controls to respond to an incident"@en .

risk-owl:PsychologicalHarm a rdfs:Class,
        owl:Class,
        dpv-owl:RiskConcept,
        risk-owl:PotentialConsequence,
        risk-owl:PotentialImpact,
        risk-owl:PotentialRisk ;
    dct:contributor _:Ne22a67b17c7e4a779c30d2864b6a0cee ;
    dct:created "2022-08-17"^^xsd:date ;
    dct:modified "2024-08-16"^^xsd:date ;
    dct:source [ a schema:WebPage ;
            schema:name "ENISA Reference Incident Classification Taxonomy 2018" ;
            schema:url "https://www.enisa.europa.eu/publications/reference-incident-classification-taxonomy/" ] ;
    rdfs:isDefinedBy risk-owl: ;
    rdfs:subClassOf risk-owl:Harm,
        risk-owl:MentalSafety,
        risk-owl:Wellbeing ;
    sw:term_status "accepted"@en ;
    skos:definition "Concept representing Psychological Harm"@en ;
    skos:prefLabel "Psychological Harm"@en .

risk-owl:PublicHealthSafety a rdfs:Class,
        owl:Class,
        dpv-owl:RiskConcept,
        risk-owl:PotentialConsequence,
        risk-owl:PotentialImpact,
        risk-owl:PotentialRisk ;
    dct:created "2024-12-01"^^xsd:date ;
    rdfs:isDefinedBy risk-owl: ;
    rdfs:subClassOf risk-owl:HealthSafety ;
    sw:term_status "accepted"@en ;
    skos:definition "Concept representing health and safety of the public at large"@en ;
    skos:prefLabel "Public Health & Safety"@en .

risk-owl:PublicOrderBreach a rdfs:Class,
        owl:Class,
        dpv-owl:RiskConcept,
        risk-owl:PotentialConsequence,
        risk-owl:PotentialRisk ;
    dct:contributor _:Ne22a67b17c7e4a779c30d2864b6a0cee ;
    dct:created "2022-08-17"^^xsd:date ;
    dct:modified "2024-08-16"^^xsd:date ;
    dct:source [ a schema:WebPage ;
            schema:name "ISO/IEC 27005:2018" ;
            schema:url "https://www.iso.org/standard/75281.html" ] ;
    rdfs:isDefinedBy risk-owl: ;
    rdfs:subClassOf risk-owl:LegalComplianceRisk ;
    sw:term_status "accepted"@en ;
    skos:definition "Concept representing Public Order Breach"@en ;
    skos:prefLabel "Public Order Breach"@en .

risk-owl:PublicServicesExclusion a rdfs:Class,
        owl:Class,
        dpv-owl:RiskConcept,
        risk-owl:PotentialConsequence,
        risk-owl:PotentialImpact,
        risk-owl:PotentialRisk ;
    dct:created "2024-10-21"^^xsd:date ;
    rdfs:isDefinedBy risk-owl: ;
    rdfs:subClassOf risk-owl:ServiceRelatedConsequence ;
    sw:term_status "accepted"@en ;
    skos:definition "Concept representing exclusion from public services"@en ;
    skos:prefLabel "Public Services Exclusion"@en .

risk-owl:QualityDegraded a rdfs:Class,
        owl:Class,
        dpv-owl:RiskConcept,
        risk-owl:PotentialConsequence,
        risk-owl:PotentialRisk,
        risk-owl:PotentialRiskSource ;
    dct:contributor _:Ne22a67b17c7e4a779c30d2864b6a0cee ;
    dct:created "2024-12-01"^^xsd:date ;
    rdfs:isDefinedBy risk-owl: ;
    rdfs:subClassOf risk-owl:QualityRisk ;
    sw:term_status "accepted"@en ;
    skos:definition "Concepts representing risks and issues where Quality is Degraded"@en ;
    skos:prefLabel "Quality Degraded"@en .

risk-owl:QualityInconsistent a rdfs:Class,
        owl:Class,
        dpv-owl:RiskConcept,
        risk-owl:PotentialConsequence,
        risk-owl:PotentialRisk,
        risk-owl:PotentialRiskSource ;
    dct:contributor _:Ne22a67b17c7e4a779c30d2864b6a0cee ;
    dct:created "2024-12-01"^^xsd:date ;
    rdfs:isDefinedBy risk-owl: ;
    rdfs:subClassOf risk-owl:QualityRisk ;
    sw:term_status "accepted"@en ;
    skos:definition "Concepts representing risks and issues where Quality is Inconsistent"@en ;
    skos:prefLabel "Quality Inconsistent"@en .

risk-owl:QualityInsufficient a rdfs:Class,
        owl:Class,
        dpv-owl:RiskConcept,
        risk-owl:PotentialConsequence,
        risk-owl:PotentialRisk,
        risk-owl:PotentialRiskSource ;
    dct:contributor _:Ne22a67b17c7e4a779c30d2864b6a0cee ;
    dct:created "2024-12-01"^^xsd:date ;
    rdfs:isDefinedBy risk-owl: ;
    rdfs:subClassOf risk-owl:QualityRisk ;
    sw:term_status "accepted"@en ;
    skos:definition "Concepts representing risks and issues where Quality is Insufficient"@en ;
    skos:prefLabel "Quality Insufficient"@en .

risk-owl:QualityRisk a rdfs:Class,
        owl:Class,
        dpv-owl:RiskConcept,
        risk-owl:PotentialConsequence,
        risk-owl:PotentialRisk,
        risk-owl:PotentialRiskSource ;
    dct:contributor _:Ne22a67b17c7e4a779c30d2864b6a0cee ;
    dct:created "2024-12-01"^^xsd:date ;
    rdfs:isDefinedBy risk-owl: ;
    rdfs:subClassOf risk-owl:OperationalSecurityRisk ;
    sw:term_status "accepted"@en ;
    skos:definition "Concept representing risks and issues associated with quality of tasks, resources, processes"@en ;
    skos:prefLabel "Quality Risk"@en .

risk-owl:QualityUnknown a rdfs:Class,
        owl:Class,
        dpv-owl:RiskConcept,
        risk-owl:PotentialConsequence,
        risk-owl:PotentialRisk,
        risk-owl:PotentialRiskSource ;
    dct:contributor _:Ne22a67b17c7e4a779c30d2864b6a0cee ;
    dct:created "2024-12-01"^^xsd:date ;
    rdfs:isDefinedBy risk-owl: ;
    rdfs:subClassOf risk-owl:QualityRisk ;
    sw:term_status "accepted"@en ;
    skos:definition "Concepts representing risks and issues where Quality is Unknown"@en ;
    skos:prefLabel "Quality Unknown"@en .

risk-owl:QualityUnverified a rdfs:Class,
        owl:Class,
        dpv-owl:RiskConcept,
        risk-owl:PotentialConsequence,
        risk-owl:PotentialRisk,
        risk-owl:PotentialRiskSource ;
    dct:contributor _:Ne22a67b17c7e4a779c30d2864b6a0cee ;
    dct:created "2024-12-01"^^xsd:date ;
    rdfs:isDefinedBy risk-owl: ;
    rdfs:subClassOf risk-owl:QualityRisk ;
    sw:term_status "accepted"@en ;
    skos:definition "Concepts representing risks and issues where Quality is Unverified"@en ;
    skos:prefLabel "Quality Unverified"@en .

risk-owl:RM3x3S1L1 a rdfs:Class,
        owl:Class,
        risk-owl:RiskAnalysis ;
    dct:contributor _:Ne22a67b17c7e4a779c30d2864b6a0cee ;
    dct:created "2022-08-17"^^xsd:date ;
    rdf:value "0.11,xsd:decimal" ;
    rdfs:isDefinedBy risk-owl: ;
    rdfs:subClassOf risk-owl:RiskMatrix3x3 ;
    sw:term_status "accepted"@en ;
    skos:definition "Node in a 3x3 Risk Matrix with Risk Severity: Low; Likelihood: Low; and Risk Level: Low"@en ;
    skos:prefLabel "Low Risk (RM3x3 S:1 L:1)"@en .

risk-owl:RM3x3S1L2 a rdfs:Class,
        owl:Class,
        risk-owl:RiskAnalysis ;
    dct:contributor _:Ne22a67b17c7e4a779c30d2864b6a0cee ;
    dct:created "2022-08-17"^^xsd:date ;
    rdf:value "0.22,xsd:decimal" ;
    rdfs:isDefinedBy risk-owl: ;
    rdfs:subClassOf risk-owl:RiskMatrix3x3 ;
    sw:term_status "accepted"@en ;
    skos:definition "Node in a 3x3 Risk Matrix with Risk Severity: Low; Likelihood: Moderate; and Risk Level: Low"@en ;
    skos:prefLabel "Low Risk (RM3x3 S:1 L:2)"@en .

risk-owl:RM3x3S1L3 a rdfs:Class,
        owl:Class,
        risk-owl:RiskAnalysis ;
    dct:contributor _:Ne22a67b17c7e4a779c30d2864b6a0cee ;
    dct:created "2022-08-17"^^xsd:date ;
    rdf:value "0.33,xsd:decimal" ;
    rdfs:isDefinedBy risk-owl: ;
    rdfs:subClassOf risk-owl:RiskMatrix3x3 ;
    sw:term_status "accepted"@en ;
    skos:definition "Node in a 3x3 Risk Matrix with Risk Severity: Low; Likelihood: High; and Risk Level: Moderate"@en ;
    skos:prefLabel "Moderate Risk (RM3x3 S:1 L:3)"@en .

risk-owl:RM3x3S2L1 a rdfs:Class,
        owl:Class,
        risk-owl:RiskAnalysis ;
    dct:contributor _:Ne22a67b17c7e4a779c30d2864b6a0cee ;
    dct:created "2022-08-17"^^xsd:date ;
    rdf:value "0.22,xsd:decimal" ;
    rdfs:isDefinedBy risk-owl: ;
    rdfs:subClassOf risk-owl:RiskMatrix3x3 ;
    sw:term_status "accepted"@en ;
    skos:definition "Node in a 3x3 Risk Matrix with Risk Severity: Moderate; Likelihood: Low; and Risk Level: Low"@en ;
    skos:prefLabel "Low Risk (RM3x3 S:2 L:1)"@en .

risk-owl:RM3x3S2L2 a rdfs:Class,
        owl:Class,
        risk-owl:RiskAnalysis ;
    dct:contributor _:Ne22a67b17c7e4a779c30d2864b6a0cee ;
    dct:created "2022-08-17"^^xsd:date ;
    rdf:value "0.44,xsd:decimal" ;
    rdfs:isDefinedBy risk-owl: ;
    rdfs:subClassOf risk-owl:RiskMatrix3x3 ;
    sw:term_status "accepted"@en ;
    skos:definition "Node in a 3x3 Risk Matrix with Risk Severity: Moderate; Likelihood: Moderate; and Risk Level: Moderate"@en ;
    skos:prefLabel "Moderate Risk (RM3x3 S:2 L:2)"@en .

risk-owl:RM3x3S2L3 a rdfs:Class,
        owl:Class,
        risk-owl:RiskAnalysis ;
    dct:contributor _:Ne22a67b17c7e4a779c30d2864b6a0cee ;
    dct:created "2022-08-17"^^xsd:date ;
    rdf:value "0.67,xsd:decimal" ;
    rdfs:isDefinedBy risk-owl: ;
    rdfs:subClassOf risk-owl:RiskMatrix3x3 ;
    sw:term_status "accepted"@en ;
    skos:definition "Node in a 3x3 Risk Matrix with Risk Severity: Moderate; Likelihood: High; and Risk Level: High"@en ;
    skos:prefLabel "High Risk (RM3x3 S:2 L:3)"@en .

risk-owl:RM3x3S3L1 a rdfs:Class,
        owl:Class,
        risk-owl:RiskAnalysis ;
    dct:contributor _:Ne22a67b17c7e4a779c30d2864b6a0cee ;
    dct:created "2022-08-17"^^xsd:date ;
    rdf:value "0.33,xsd:decimal" ;
    rdfs:isDefinedBy risk-owl: ;
    rdfs:subClassOf risk-owl:RiskMatrix3x3 ;
    sw:term_status "accepted"@en ;
    skos:definition "Node in a 3x3 Risk Matrix with Risk Severity: High; Likelihood: Low; and Risk Level: Moderate"@en ;
    skos:prefLabel "Moderate Risk (RM3x3 S:3 L:1)"@en .

risk-owl:RM3x3S3L2 a rdfs:Class,
        owl:Class,
        risk-owl:RiskAnalysis ;
    dct:contributor _:Ne22a67b17c7e4a779c30d2864b6a0cee ;
    dct:created "2022-08-17"^^xsd:date ;
    rdf:value "0.67,xsd:decimal" ;
    rdfs:isDefinedBy risk-owl: ;
    rdfs:subClassOf risk-owl:RiskMatrix3x3 ;
    sw:term_status "accepted"@en ;
    skos:definition "Node in a 3x3 Risk Matrix with Risk Severity: High; Likelihood: Moderate; and Risk Level: High"@en ;
    skos:prefLabel "High Risk (RM3x3 S:3 L:2)"@en .

risk-owl:RM3x3S3L3 a rdfs:Class,
        owl:Class,
        risk-owl:RiskAnalysis ;
    dct:contributor _:Ne22a67b17c7e4a779c30d2864b6a0cee ;
    dct:created "2022-08-17"^^xsd:date ;
    rdf:value "0.99,xsd:decimal" ;
    rdfs:isDefinedBy risk-owl: ;
    rdfs:subClassOf risk-owl:RiskMatrix3x3 ;
    sw:term_status "accepted"@en ;
    skos:definition "Node in a 3x3 Risk Matrix with Risk Severity: High; Likelihood: High; and Risk Level: High"@en ;
    skos:prefLabel "High Risk (RM3x3 S:3 L:3)"@en .

risk-owl:RM5x5S1L1 a rdfs:Class,
        owl:Class,
        risk-owl:RiskAnalysis ;
    dct:contributor _:Ne22a67b17c7e4a779c30d2864b6a0cee ;
    dct:created "2022-08-17"^^xsd:date ;
    rdf:value "0.04,xsd:decimal" ;
    rdfs:isDefinedBy risk-owl: ;
    rdfs:subClassOf risk-owl:RiskMatrix5x5 ;
    sw:term_status "accepted"@en ;
    skos:definition "Node in a 5x5 Risk Matrix with Risk Severity: Very Low; Likelihood: Very Low; and Risk Level: Very Low"@en ;
    skos:prefLabel "Very Low Risk (RM5x5 S:1 L:1)"@en .

risk-owl:RM5x5S1L2 a rdfs:Class,
        owl:Class,
        risk-owl:RiskAnalysis ;
    dct:contributor _:Ne22a67b17c7e4a779c30d2864b6a0cee ;
    dct:created "2022-08-17"^^xsd:date ;
    rdf:value "0.08,xsd:decimal" ;
    rdfs:isDefinedBy risk-owl: ;
    rdfs:subClassOf risk-owl:RiskMatrix5x5 ;
    sw:term_status "accepted"@en ;
    skos:definition "Node in a 5x5 Risk Matrix with Risk Severity: Very Low; Likelihood: Low; and Risk Level: Very Low"@en ;
    skos:prefLabel "Very Low Risk (RM5x5 S:1 L:2)"@en .

risk-owl:RM5x5S1L3 a rdfs:Class,
        owl:Class,
        risk-owl:RiskAnalysis ;
    dct:contributor _:Ne22a67b17c7e4a779c30d2864b6a0cee ;
    dct:created "2022-08-17"^^xsd:date ;
    rdf:value "0.12,xsd:decimal" ;
    rdfs:isDefinedBy risk-owl: ;
    rdfs:subClassOf risk-owl:RiskMatrix5x5 ;
    sw:term_status "accepted"@en ;
    skos:definition "Node in a 5x5 Risk Matrix with Risk Severity: Very Low; Likelihood: Moderate; and Risk Level: Very Low"@en ;
    skos:prefLabel "Very Low Risk (RM5x5 S:1 L:3)"@en .

risk-owl:RM5x5S1L4 a rdfs:Class,
        owl:Class,
        risk-owl:RiskAnalysis ;
    dct:contributor _:Ne22a67b17c7e4a779c30d2864b6a0cee ;
    dct:created "2022-08-17"^^xsd:date ;
    rdf:value "0.16,xsd:decimal" ;
    rdfs:isDefinedBy risk-owl: ;
    rdfs:subClassOf risk-owl:RiskMatrix5x5 ;
    sw:term_status "accepted"@en ;
    skos:definition "Node in a 5x5 Risk Matrix with Risk Severity: Very Low; Likelihood: High; and Risk Level: Low"@en ;
    skos:prefLabel "Low Risk (RM5x5 S:1 L:4)"@en .

risk-owl:RM5x5S1L5 a rdfs:Class,
        owl:Class,
        risk-owl:RiskAnalysis ;
    dct:contributor _:Ne22a67b17c7e4a779c30d2864b6a0cee ;
    dct:created "2022-08-17"^^xsd:date ;
    rdf:value "0.20,xsd:decimal" ;
    rdfs:isDefinedBy risk-owl: ;
    rdfs:subClassOf risk-owl:RiskMatrix5x5 ;
    sw:term_status "accepted"@en ;
    skos:definition "Node in a 5x5 Risk Matrix with Risk Severity: Very Low; Likelihood: Very High; and Risk Level: Low"@en ;
    skos:prefLabel "Low Risk (RM5x5 S:1 L:5)"@en .

risk-owl:RM5x5S2L1 a rdfs:Class,
        owl:Class,
        risk-owl:RiskAnalysis ;
    dct:contributor _:Ne22a67b17c7e4a779c30d2864b6a0cee ;
    dct:created "2022-08-17"^^xsd:date ;
    rdf:value "0.08,xsd:decimal" ;
    rdfs:isDefinedBy risk-owl: ;
    rdfs:subClassOf risk-owl:RiskMatrix5x5 ;
    sw:term_status "accepted"@en ;
    skos:definition "Node in a 5x5 Risk Matrix with Risk Severity: Low; Likelihood: Very Low; and Risk Level: Very Low"@en ;
    skos:prefLabel "Very Low Risk (RM5x5 S:2 L:1)"@en .

risk-owl:RM5x5S2L2 a rdfs:Class,
        owl:Class,
        risk-owl:RiskAnalysis ;
    dct:contributor _:Ne22a67b17c7e4a779c30d2864b6a0cee ;
    dct:created "2022-08-17"^^xsd:date ;
    rdf:value "0.16,xsd:decimal" ;
    rdfs:isDefinedBy risk-owl: ;
    rdfs:subClassOf risk-owl:RiskMatrix5x5 ;
    sw:term_status "accepted"@en ;
    skos:definition "Node in a 5x5 Risk Matrix with Risk Severity: Low; Likelihood: Low; and Risk Level: Low"@en ;
    skos:prefLabel "Low Risk (RM5x5 S:2 L:2)"@en .

risk-owl:RM5x5S2L3 a rdfs:Class,
        owl:Class,
        risk-owl:RiskAnalysis ;
    dct:contributor _:Ne22a67b17c7e4a779c30d2864b6a0cee ;
    dct:created "2022-08-17"^^xsd:date ;
    rdf:value "0.24,xsd:decimal" ;
    rdfs:isDefinedBy risk-owl: ;
    rdfs:subClassOf risk-owl:RiskMatrix5x5 ;
    sw:term_status "accepted"@en ;
    skos:definition "Node in a 5x5 Risk Matrix with Risk Severity: Low; Likelihood: Moderate; and Risk Level: Moderate"@en ;
    skos:prefLabel "Moderate Risk (RM5x5 S:2 L:3)"@en .

risk-owl:RM5x5S2L4 a rdfs:Class,
        owl:Class,
        risk-owl:RiskAnalysis ;
    dct:contributor _:Ne22a67b17c7e4a779c30d2864b6a0cee ;
    dct:created "2022-08-17"^^xsd:date ;
    rdf:value "0.32,xsd:decimal" ;
    rdfs:isDefinedBy risk-owl: ;
    rdfs:subClassOf risk-owl:RiskMatrix5x5 ;
    sw:term_status "accepted"@en ;
    skos:definition "Node in a 5x5 Risk Matrix with Risk Severity: Low; Likelihood: High; and Risk Level: Moderate"@en ;
    skos:prefLabel "Moderate Risk (RM5x5 S:2 L:4)"@en .

risk-owl:RM5x5S2L5 a rdfs:Class,
        owl:Class,
        risk-owl:RiskAnalysis ;
    dct:contributor _:Ne22a67b17c7e4a779c30d2864b6a0cee ;
    dct:created "2022-08-17"^^xsd:date ;
    rdf:value "0.40,xsd:decimal" ;
    rdfs:isDefinedBy risk-owl: ;
    rdfs:subClassOf risk-owl:RiskMatrix5x5 ;
    sw:term_status "accepted"@en ;
    skos:definition "Node in a 5x5 Risk Matrix with Risk Severity: Low; Likelihood: Very High; and Risk Level: High"@en ;
    skos:prefLabel "High Risk (RM5x5 S:2 L:5)"@en .

risk-owl:RM5x5S3L1 a rdfs:Class,
        owl:Class,
        risk-owl:RiskAnalysis ;
    dct:contributor _:Ne22a67b17c7e4a779c30d2864b6a0cee ;
    dct:created "2022-08-17"^^xsd:date ;
    rdf:value "0.12,xsd:decimal" ;
    rdfs:isDefinedBy risk-owl: ;
    rdfs:subClassOf risk-owl:RiskMatrix5x5 ;
    sw:term_status "accepted"@en ;
    skos:definition "Node in a 5x5 Risk Matrix with Risk Severity: Moderate; Likelihood: Very Low; and Risk Level: Very Low"@en ;
    skos:prefLabel "Very Low Risk (RM5x5 S:3 L:1)"@en .

risk-owl:RM5x5S3L2 a rdfs:Class,
        owl:Class,
        risk-owl:RiskAnalysis ;
    dct:contributor _:Ne22a67b17c7e4a779c30d2864b6a0cee ;
    dct:created "2022-08-17"^^xsd:date ;
    rdf:value "0.24,xsd:decimal" ;
    rdfs:isDefinedBy risk-owl: ;
    rdfs:subClassOf risk-owl:RiskMatrix5x5 ;
    sw:term_status "accepted"@en ;
    skos:definition "Node in a 5x5 Risk Matrix with Risk Severity: Moderate; Likelihood: Low; and Risk Level: Moderate"@en ;
    skos:prefLabel "Moderate Risk (RM5x5 S:3 L:2)"@en .

risk-owl:RM5x5S3L3 a rdfs:Class,
        owl:Class,
        risk-owl:RiskAnalysis ;
    dct:contributor _:Ne22a67b17c7e4a779c30d2864b6a0cee ;
    dct:created "2022-08-17"^^xsd:date ;
    rdf:value "0.36,xsd:decimal" ;
    rdfs:isDefinedBy risk-owl: ;
    rdfs:subClassOf risk-owl:RiskMatrix5x5 ;
    sw:term_status "accepted"@en ;
    skos:definition "Node in a 5x5 Risk Matrix with Risk Severity: Moderate; Likelihood: Moderate; and Risk Level: Moderate"@en ;
    skos:prefLabel "Moderate Risk (RM5x5 S:3 L:3)"@en .

risk-owl:RM5x5S3L4 a rdfs:Class,
        owl:Class,
        risk-owl:RiskAnalysis ;
    dct:contributor _:Ne22a67b17c7e4a779c30d2864b6a0cee ;
    dct:created "2022-08-17"^^xsd:date ;
    rdf:value "0.48,xsd:decimal" ;
    rdfs:isDefinedBy risk-owl: ;
    rdfs:subClassOf risk-owl:RiskMatrix5x5 ;
    sw:term_status "accepted"@en ;
    skos:definition "Node in a 5x5 Risk Matrix with Risk Severity: Moderate; Likelihood: High; and Risk Level: High"@en ;
    skos:prefLabel "High Risk (RM5x5 S:3 L:4)"@en .

risk-owl:RM5x5S3L5 a rdfs:Class,
        owl:Class,
        risk-owl:RiskAnalysis ;
    dct:contributor _:Ne22a67b17c7e4a779c30d2864b6a0cee ;
    dct:created "2022-08-17"^^xsd:date ;
    rdf:value "0.60,xsd:decimal" ;
    rdfs:isDefinedBy risk-owl: ;
    rdfs:subClassOf risk-owl:RiskMatrix5x5 ;
    sw:term_status "accepted"@en ;
    skos:definition "Node in a 5x5 Risk Matrix with Risk Severity: Moderate; Likelihood: Very High; and Risk Level: Very High"@en ;
    skos:prefLabel "Very High Risk (RM5x5 S:3 L:5)"@en .

risk-owl:RM5x5S4L1 a rdfs:Class,
        owl:Class,
        risk-owl:RiskAnalysis ;
    dct:contributor _:Ne22a67b17c7e4a779c30d2864b6a0cee ;
    dct:created "2022-08-17"^^xsd:date ;
    rdf:value "0.16,xsd:decimal" ;
    rdfs:isDefinedBy risk-owl: ;
    rdfs:subClassOf risk-owl:RiskMatrix5x5 ;
    sw:term_status "accepted"@en ;
    skos:definition "Node in a 5x5 Risk Matrix with Risk Severity: High; Likelihood: Very Low; and Risk Level: Low"@en ;
    skos:prefLabel "Low Risk (RM5x5 S:4 L:1)"@en .

risk-owl:RM5x5S4L2 a rdfs:Class,
        owl:Class,
        risk-owl:RiskAnalysis ;
    dct:contributor _:Ne22a67b17c7e4a779c30d2864b6a0cee ;
    dct:created "2022-08-17"^^xsd:date ;
    rdf:value "0.32,xsd:decimal" ;
    rdfs:isDefinedBy risk-owl: ;
    rdfs:subClassOf risk-owl:RiskMatrix5x5 ;
    sw:term_status "accepted"@en ;
    skos:definition "Node in a 5x5 Risk Matrix with Risk Severity: High; Likelihood: Low; and Risk Level: Moderate"@en ;
    skos:prefLabel "Moderate Risk (RM5x5 S:4 L:2)"@en .

risk-owl:RM5x5S4L3 a rdfs:Class,
        owl:Class,
        risk-owl:RiskAnalysis ;
    dct:contributor _:Ne22a67b17c7e4a779c30d2864b6a0cee ;
    dct:created "2022-08-17"^^xsd:date ;
    rdf:value "0.48,xsd:decimal" ;
    rdfs:isDefinedBy risk-owl: ;
    rdfs:subClassOf risk-owl:RiskMatrix5x5 ;
    sw:term_status "accepted"@en ;
    skos:definition "Node in a 5x5 Risk Matrix with Risk Severity: High; Likelihood: Moderate; and Risk Level: High"@en ;
    skos:prefLabel "High Risk (RM5x5 S:4 L:3)"@en .

risk-owl:RM5x5S4L4 a rdfs:Class,
        owl:Class,
        risk-owl:RiskAnalysis ;
    dct:contributor _:Ne22a67b17c7e4a779c30d2864b6a0cee ;
    dct:created "2022-08-17"^^xsd:date ;
    rdf:value "0.64,xsd:decimal" ;
    rdfs:isDefinedBy risk-owl: ;
    rdfs:subClassOf risk-owl:RiskMatrix5x5 ;
    sw:term_status "accepted"@en ;
    skos:definition "Node in a 5x5 Risk Matrix with Risk Severity: High; Likelihood: High; and Risk Level: Very High"@en ;
    skos:prefLabel "Very High Risk (RM5x5 S:4 L:4)"@en .

risk-owl:RM5x5S4L5 a rdfs:Class,
        owl:Class,
        risk-owl:RiskAnalysis ;
    dct:contributor _:Ne22a67b17c7e4a779c30d2864b6a0cee ;
    dct:created "2022-08-17"^^xsd:date ;
    rdf:value "0.80,xsd:decimal" ;
    rdfs:isDefinedBy risk-owl: ;
    rdfs:subClassOf risk-owl:RiskMatrix5x5 ;
    sw:term_status "accepted"@en ;
    skos:definition "Node in a 5x5 Risk Matrix with Risk Severity: High; Likelihood: Very High; and Risk Level: Very High"@en ;
    skos:prefLabel "Very High Risk (RM5x5 S:4 L:5)"@en .

risk-owl:RM5x5S5L1 a rdfs:Class,
        owl:Class,
        risk-owl:RiskAnalysis ;
    dct:contributor _:Ne22a67b17c7e4a779c30d2864b6a0cee ;
    dct:created "2022-08-17"^^xsd:date ;
    rdf:value "0.20,xsd:decimal" ;
    rdfs:isDefinedBy risk-owl: ;
    rdfs:subClassOf risk-owl:RiskMatrix5x5 ;
    sw:term_status "accepted"@en ;
    skos:definition "Node in a 5x5 Risk Matrix with Risk Severity: Very High; Likelihood: Very Low; and Risk Level: Low"@en ;
    skos:prefLabel "Low Risk (RM5x5 S:5 L:1)"@en .

risk-owl:RM5x5S5L2 a rdfs:Class,
        owl:Class,
        risk-owl:RiskAnalysis ;
    dct:contributor _:Ne22a67b17c7e4a779c30d2864b6a0cee ;
    dct:created "2022-08-17"^^xsd:date ;
    rdf:value "0.40,xsd:decimal" ;
    rdfs:isDefinedBy risk-owl: ;
    rdfs:subClassOf risk-owl:RiskMatrix5x5 ;
    sw:term_status "accepted"@en ;
    skos:definition "Node in a 5x5 Risk Matrix with Risk Severity: Very High; Likelihood: Low; and Risk Level: High"@en ;
    skos:prefLabel "High Risk (RM5x5 S:5 L:2)"@en .

risk-owl:RM5x5S5L3 a rdfs:Class,
        owl:Class,
        risk-owl:RiskAnalysis ;
    dct:contributor _:Ne22a67b17c7e4a779c30d2864b6a0cee ;
    dct:created "2022-08-17"^^xsd:date ;
    rdf:value "0.60,xsd:decimal" ;
    rdfs:isDefinedBy risk-owl: ;
    rdfs:subClassOf risk-owl:RiskMatrix5x5 ;
    sw:term_status "accepted"@en ;
    skos:definition "Node in a 5x5 Risk Matrix with Risk Severity: Very High; Likelihood: Moderate; and Risk Level: High"@en ;
    skos:prefLabel "High Risk (RM5x5 S:5 L:3)"@en .

risk-owl:RM5x5S5L4 a rdfs:Class,
        owl:Class,
        risk-owl:RiskAnalysis ;
    dct:contributor _:Ne22a67b17c7e4a779c30d2864b6a0cee ;
    dct:created "2022-08-17"^^xsd:date ;
    rdf:value "0.80,xsd:decimal" ;
    rdfs:isDefinedBy risk-owl: ;
    rdfs:subClassOf risk-owl:RiskMatrix5x5 ;
    sw:term_status "accepted"@en ;
    skos:definition "Node in a 5x5 Risk Matrix with Risk Severity: Very High; Likelihood: High; and Risk Level: Very High"@en ;
    skos:prefLabel "Very High Risk (RM5x5 S:5 L:4)"@en .

risk-owl:RM5x5S5L5 a rdfs:Class,
        owl:Class,
        risk-owl:RiskAnalysis ;
    dct:contributor _:Ne22a67b17c7e4a779c30d2864b6a0cee ;
    dct:created "2022-08-17"^^xsd:date ;
    rdf:value "0.99,xsd:decimal" ;
    rdfs:isDefinedBy risk-owl: ;
    rdfs:subClassOf risk-owl:RiskMatrix5x5 ;
    sw:term_status "accepted"@en ;
    skos:definition "Node in a 5x5 Risk Matrix with Risk Severity: Very High; Likelihood: Very High; and Risk Level: Very High"@en ;
    skos:prefLabel "Very High Risk (RM5x5 S:5 L:5)"@en .

risk-owl:RM7x7S1L1 a rdfs:Class,
        owl:Class,
        risk-owl:RiskAnalysis ;
    dct:contributor _:Ne22a67b17c7e4a779c30d2864b6a0cee ;
    dct:created "2022-08-17"^^xsd:date ;
    rdf:value "0.02,xsd:decimal" ;
    rdfs:isDefinedBy risk-owl: ;
    rdfs:subClassOf risk-owl:RiskMatrix7x7 ;
    sw:term_status "accepted"@en ;
    skos:definition "Node in a 7x7 Risk Matrix with Risk Severity: Extremely Low; Likelihood: Extremely Low; and Risk Level: Extremely Low"@en ;
    skos:prefLabel "Extremely Low Risk (RM7x7 S:1 L:1)"@en .

risk-owl:RM7x7S1L2 a rdfs:Class,
        owl:Class,
        risk-owl:RiskAnalysis ;
    dct:contributor _:Ne22a67b17c7e4a779c30d2864b6a0cee ;
    dct:created "2022-08-17"^^xsd:date ;
    rdf:value "0.04,xsd:decimal" ;
    rdfs:isDefinedBy risk-owl: ;
    rdfs:subClassOf risk-owl:RiskMatrix7x7 ;
    sw:term_status "accepted"@en ;
    skos:definition "Node in a 7x7 Risk Matrix with Risk Severity: Extremely Low; Likelihood: Very Low; and Risk Level: Extremely Low"@en ;
    skos:prefLabel "Extremely Low Risk (RM7x7 S:1 L:2)"@en .

risk-owl:RM7x7S1L3 a rdfs:Class,
        owl:Class,
        risk-owl:RiskAnalysis ;
    dct:contributor _:Ne22a67b17c7e4a779c30d2864b6a0cee ;
    dct:created "2022-08-17"^^xsd:date ;
    rdf:value "0.06,xsd:decimal" ;
    rdfs:isDefinedBy risk-owl: ;
    rdfs:subClassOf risk-owl:RiskMatrix7x7 ;
    sw:term_status "accepted"@en ;
    skos:definition "Node in a 7x7 Risk Matrix with Risk Severity: Extremely Low; Likelihood: Low; and Risk Level: Extremely Low"@en ;
    skos:prefLabel "Extremely Low Risk (RM7x7 S:1 L:3)"@en .

risk-owl:RM7x7S1L4 a rdfs:Class,
        owl:Class,
        risk-owl:RiskAnalysis ;
    dct:contributor _:Ne22a67b17c7e4a779c30d2864b6a0cee ;
    dct:created "2022-08-17"^^xsd:date ;
    rdf:value "0.08,xsd:decimal" ;
    rdfs:isDefinedBy risk-owl: ;
    rdfs:subClassOf risk-owl:RiskMatrix7x7 ;
    sw:term_status "accepted"@en ;
    skos:definition "Node in a 7x7 Risk Matrix with Risk Severity: Extremely Low; Likelihood: Moderate; and Risk Level: Very Low"@en ;
    skos:prefLabel "Very Low Risk (RM7x7 S:1 L:4)"@en .

risk-owl:RM7x7S1L5 a rdfs:Class,
        owl:Class,
        risk-owl:RiskAnalysis ;
    dct:contributor _:Ne22a67b17c7e4a779c30d2864b6a0cee ;
    dct:created "2022-08-17"^^xsd:date ;
    rdf:value "0.10,xsd:decimal" ;
    rdfs:isDefinedBy risk-owl: ;
    rdfs:subClassOf risk-owl:RiskMatrix7x7 ;
    sw:term_status "accepted"@en ;
    skos:definition "Node in a 7x7 Risk Matrix with Risk Severity: Extremely Low; Likelihood: High; and Risk Level: Very Low"@en ;
    skos:prefLabel "Very Low Risk (RM7x7 S:1 L:5)"@en .

risk-owl:RM7x7S1L6 a rdfs:Class,
        owl:Class,
        risk-owl:RiskAnalysis ;
    dct:contributor _:Ne22a67b17c7e4a779c30d2864b6a0cee ;
    dct:created "2022-08-17"^^xsd:date ;
    rdf:value "0.12,xsd:decimal" ;
    rdfs:isDefinedBy risk-owl: ;
    rdfs:subClassOf risk-owl:RiskMatrix7x7 ;
    sw:term_status "accepted"@en ;
    skos:definition "Node in a 7x7 Risk Matrix with Risk Severity: Extremely Low; Likelihood: Very High; and Risk Level: Very Low"@en ;
    skos:prefLabel "Very Low Risk (RM7x7 S:1 L:6)"@en .

risk-owl:RM7x7S1L7 a rdfs:Class,
        owl:Class,
        risk-owl:RiskAnalysis ;
    dct:contributor _:Ne22a67b17c7e4a779c30d2864b6a0cee ;
    dct:created "2022-08-17"^^xsd:date ;
    rdf:value "0.14,xsd:decimal" ;
    rdfs:isDefinedBy risk-owl: ;
    rdfs:subClassOf risk-owl:RiskMatrix7x7 ;
    sw:term_status "accepted"@en ;
    skos:definition "Node in a 7x7 Risk Matrix with Risk Severity: Extremely Low; Likelihood: Extremely High; and Risk Level: Low"@en ;
    skos:prefLabel "Low Risk (RM7x7 S:1 L:7)"@en .

risk-owl:RM7x7S2L1 a rdfs:Class,
        owl:Class,
        risk-owl:RiskAnalysis ;
    dct:contributor _:Ne22a67b17c7e4a779c30d2864b6a0cee ;
    dct:created "2022-08-17"^^xsd:date ;
    rdf:value "0.04,xsd:decimal" ;
    rdfs:isDefinedBy risk-owl: ;
    rdfs:subClassOf risk-owl:RiskMatrix7x7 ;
    sw:term_status "accepted"@en ;
    skos:definition "Node in a 7x7 Risk Matrix with Risk Severity: Very Low; Likelihood: Extremely Low; and Risk Level: Extremely Low"@en ;
    skos:prefLabel "Extremely Low Risk (RM7x7 S:2 L:1)"@en .

risk-owl:RM7x7S2L2 a rdfs:Class,
        owl:Class,
        risk-owl:RiskAnalysis ;
    dct:contributor _:Ne22a67b17c7e4a779c30d2864b6a0cee ;
    dct:created "2022-08-17"^^xsd:date ;
    rdf:value "0.08,xsd:decimal" ;
    rdfs:isDefinedBy risk-owl: ;
    rdfs:subClassOf risk-owl:RiskMatrix7x7 ;
    sw:term_status "accepted"@en ;
    skos:definition "Node in a 7x7 Risk Matrix with Risk Severity: Very Low; Likelihood: Very Low; and Risk Level: Extremely Low"@en ;
    skos:prefLabel "Extremely Low Risk (RM7x7 S:2 L:2)"@en .

risk-owl:RM7x7S2L3 a rdfs:Class,
        owl:Class,
        risk-owl:RiskAnalysis ;
    dct:contributor _:Ne22a67b17c7e4a779c30d2864b6a0cee ;
    dct:created "2022-08-17"^^xsd:date ;
    rdf:value "0.12,xsd:decimal" ;
    rdfs:isDefinedBy risk-owl: ;
    rdfs:subClassOf risk-owl:RiskMatrix7x7 ;
    sw:term_status "accepted"@en ;
    skos:definition "Node in a 7x7 Risk Matrix with Risk Severity: Very Low; Likelihood: Low; and Risk Level: Very Low"@en ;
    skos:prefLabel "Very Low Risk (RM7x7 S:2 L:3)"@en .

risk-owl:RM7x7S2L4 a rdfs:Class,
        owl:Class,
        risk-owl:RiskAnalysis ;
    dct:contributor _:Ne22a67b17c7e4a779c30d2864b6a0cee ;
    dct:created "2022-08-17"^^xsd:date ;
    rdf:value "0.16,xsd:decimal" ;
    rdfs:isDefinedBy risk-owl: ;
    rdfs:subClassOf risk-owl:RiskMatrix7x7 ;
    sw:term_status "accepted"@en ;
    skos:definition "Node in a 7x7 Risk Matrix with Risk Severity: Very Low; Likelihood: Moderate; and Risk Level: Low"@en ;
    skos:prefLabel "Low Risk (RM7x7 S:2 L:4)"@en .

risk-owl:RM7x7S2L5 a rdfs:Class,
        owl:Class,
        risk-owl:RiskAnalysis ;
    dct:contributor _:Ne22a67b17c7e4a779c30d2864b6a0cee ;
    dct:created "2022-08-17"^^xsd:date ;
    rdf:value "0.20,xsd:decimal" ;
    rdfs:isDefinedBy risk-owl: ;
    rdfs:subClassOf risk-owl:RiskMatrix7x7 ;
    sw:term_status "accepted"@en ;
    skos:definition "Node in a 7x7 Risk Matrix with Risk Severity: Very Low; Likelihood: High; and Risk Level: Low"@en ;
    skos:prefLabel "Low Risk (RM7x7 S:2 L:5)"@en .

risk-owl:RM7x7S2L6 a rdfs:Class,
        owl:Class,
        risk-owl:RiskAnalysis ;
    dct:contributor _:Ne22a67b17c7e4a779c30d2864b6a0cee ;
    dct:created "2022-08-17"^^xsd:date ;
    rdf:value "0.24,xsd:decimal" ;
    rdfs:isDefinedBy risk-owl: ;
    rdfs:subClassOf risk-owl:RiskMatrix7x7 ;
    sw:term_status "accepted"@en ;
    skos:definition "Node in a 7x7 Risk Matrix with Risk Severity: Very Low; Likelihood: Very High; and Risk Level: Moderate"@en ;
    skos:prefLabel "Moderate Risk (RM7x7 S:2 L:6)"@en .

risk-owl:RM7x7S2L7 a rdfs:Class,
        owl:Class,
        risk-owl:RiskAnalysis ;
    dct:contributor _:Ne22a67b17c7e4a779c30d2864b6a0cee ;
    dct:created "2022-08-17"^^xsd:date ;
    rdf:value "0.29,xsd:decimal" ;
    rdfs:isDefinedBy risk-owl: ;
    rdfs:subClassOf risk-owl:RiskMatrix7x7 ;
    sw:term_status "accepted"@en ;
    skos:definition "Node in a 7x7 Risk Matrix with Risk Severity: Very Low; Likelihood: Extremely High; and Risk Level: Moderate"@en ;
    skos:prefLabel "Moderate Risk (RM7x7 S:2 L:7)"@en .

risk-owl:RM7x7S3L1 a rdfs:Class,
        owl:Class,
        risk-owl:RiskAnalysis ;
    dct:contributor _:Ne22a67b17c7e4a779c30d2864b6a0cee ;
    dct:created "2022-08-17"^^xsd:date ;
    rdf:value "0.06,xsd:decimal" ;
    rdfs:isDefinedBy risk-owl: ;
    rdfs:subClassOf risk-owl:RiskMatrix7x7 ;
    sw:term_status "accepted"@en ;
    skos:definition "Node in a 7x7 Risk Matrix with Risk Severity: Low; Likelihood: Extremely Low; and Risk Level: Extremely Low"@en ;
    skos:prefLabel "Extremely Low Risk (RM7x7 S:3 L:1)"@en .

risk-owl:RM7x7S3L2 a rdfs:Class,
        owl:Class,
        risk-owl:RiskAnalysis ;
    dct:contributor _:Ne22a67b17c7e4a779c30d2864b6a0cee ;
    dct:created "2022-08-17"^^xsd:date ;
    rdf:value "0.12,xsd:decimal" ;
    rdfs:isDefinedBy risk-owl: ;
    rdfs:subClassOf risk-owl:RiskMatrix7x7 ;
    sw:term_status "accepted"@en ;
    skos:definition "Node in a 7x7 Risk Matrix with Risk Severity: Low; Likelihood: Very Low; and Risk Level: Very Low"@en ;
    skos:prefLabel "Very Low Risk (RM7x7 S:3 L:2)"@en .

risk-owl:RM7x7S3L3 a rdfs:Class,
        owl:Class,
        risk-owl:RiskAnalysis ;
    dct:contributor _:Ne22a67b17c7e4a779c30d2864b6a0cee ;
    dct:created "2022-08-17"^^xsd:date ;
    rdf:value "0.18,xsd:decimal" ;
    rdfs:isDefinedBy risk-owl: ;
    rdfs:subClassOf risk-owl:RiskMatrix7x7 ;
    sw:term_status "accepted"@en ;
    skos:definition "Node in a 7x7 Risk Matrix with Risk Severity: Low; Likelihood: Low; and Risk Level: Low"@en ;
    skos:prefLabel "Low Risk (RM7x7 S:3 L:3)"@en .

risk-owl:RM7x7S3L4 a rdfs:Class,
        owl:Class,
        risk-owl:RiskAnalysis ;
    dct:contributor _:Ne22a67b17c7e4a779c30d2864b6a0cee ;
    dct:created "2022-08-17"^^xsd:date ;
    rdf:value "0.24,xsd:decimal" ;
    rdfs:isDefinedBy risk-owl: ;
    rdfs:subClassOf risk-owl:RiskMatrix7x7 ;
    sw:term_status "accepted"@en ;
    skos:definition "Node in a 7x7 Risk Matrix with Risk Severity: Low; Likelihood: Moderate; and Risk Level: Moderate"@en ;
    skos:prefLabel "Moderate Risk (RM7x7 S:3 L:4)"@en .

risk-owl:RM7x7S3L5 a rdfs:Class,
        owl:Class,
        risk-owl:RiskAnalysis ;
    dct:contributor _:Ne22a67b17c7e4a779c30d2864b6a0cee ;
    dct:created "2022-08-17"^^xsd:date ;
    rdf:value "0.31,xsd:decimal" ;
    rdfs:isDefinedBy risk-owl: ;
    rdfs:subClassOf risk-owl:RiskMatrix7x7 ;
    sw:term_status "accepted"@en ;
    skos:definition "Node in a 7x7 Risk Matrix with Risk Severity: Low; Likelihood: High; and Risk Level: High"@en ;
    skos:prefLabel "High Risk (RM7x7 S:3 L:5)"@en .

risk-owl:RM7x7S3L6 a rdfs:Class,
        owl:Class,
        risk-owl:RiskAnalysis ;
    dct:contributor _:Ne22a67b17c7e4a779c30d2864b6a0cee ;
    dct:created "2022-08-17"^^xsd:date ;
    rdf:value "0.37,xsd:decimal" ;
    rdfs:isDefinedBy risk-owl: ;
    rdfs:subClassOf risk-owl:RiskMatrix7x7 ;
    sw:term_status "accepted"@en ;
    skos:definition "Node in a 7x7 Risk Matrix with Risk Severity: Low; Likelihood: Very High; and Risk Level: High"@en ;
    skos:prefLabel "High Risk (RM7x7 S:3 L:6)"@en .

risk-owl:RM7x7S3L7 a rdfs:Class,
        owl:Class,
        risk-owl:RiskAnalysis ;
    dct:contributor _:Ne22a67b17c7e4a779c30d2864b6a0cee ;
    dct:created "2022-08-17"^^xsd:date ;
    rdf:value "0.43,xsd:decimal" ;
    rdfs:isDefinedBy risk-owl: ;
    rdfs:subClassOf risk-owl:RiskMatrix7x7 ;
    sw:term_status "accepted"@en ;
    skos:definition "Node in a 7x7 Risk Matrix with Risk Severity: Low; Likelihood: Extremely High; and Risk Level: Very High"@en ;
    skos:prefLabel "Very High Risk (RM7x7 S:3 L:7)"@en .

risk-owl:RM7x7S4L1 a rdfs:Class,
        owl:Class,
        risk-owl:RiskAnalysis ;
    dct:contributor _:Ne22a67b17c7e4a779c30d2864b6a0cee ;
    dct:created "2022-08-17"^^xsd:date ;
    rdf:value "0.08,xsd:decimal" ;
    rdfs:isDefinedBy risk-owl: ;
    rdfs:subClassOf risk-owl:RiskMatrix7x7 ;
    sw:term_status "accepted"@en ;
    skos:definition "Node in a 7x7 Risk Matrix with Risk Severity: Moderate; Likelihood: Extremely Low; and Risk Level: Extremely Low"@en ;
    skos:prefLabel "Extremely Low Risk (RM7x7 S:4 L:1)"@en .

risk-owl:RM7x7S4L2 a rdfs:Class,
        owl:Class,
        risk-owl:RiskAnalysis ;
    dct:contributor _:Ne22a67b17c7e4a779c30d2864b6a0cee ;
    dct:created "2022-08-17"^^xsd:date ;
    rdf:value "0.16,xsd:decimal" ;
    rdfs:isDefinedBy risk-owl: ;
    rdfs:subClassOf risk-owl:RiskMatrix7x7 ;
    sw:term_status "accepted"@en ;
    skos:definition "Node in a 7x7 Risk Matrix with Risk Severity: Moderate; Likelihood: Very Low; and Risk Level: Low"@en ;
    skos:prefLabel "Low Risk (RM7x7 S:4 L:2)"@en .

risk-owl:RM7x7S4L3 a rdfs:Class,
        owl:Class,
        risk-owl:RiskAnalysis ;
    dct:contributor _:Ne22a67b17c7e4a779c30d2864b6a0cee ;
    dct:created "2022-08-17"^^xsd:date ;
    rdf:value "0.24,xsd:decimal" ;
    rdfs:isDefinedBy risk-owl: ;
    rdfs:subClassOf risk-owl:RiskMatrix7x7 ;
    sw:term_status "accepted"@en ;
    skos:definition "Node in a 7x7 Risk Matrix with Risk Severity: Moderate; Likelihood: Low; and Risk Level: Moderate"@en ;
    skos:prefLabel "Moderate Risk (RM7x7 S:4 L:3)"@en .

risk-owl:RM7x7S4L4 a rdfs:Class,
        owl:Class,
        risk-owl:RiskAnalysis ;
    dct:contributor _:Ne22a67b17c7e4a779c30d2864b6a0cee ;
    dct:created "2022-08-17"^^xsd:date ;
    rdf:value "0.33,xsd:decimal" ;
    rdfs:isDefinedBy risk-owl: ;
    rdfs:subClassOf risk-owl:RiskMatrix7x7 ;
    sw:term_status "accepted"@en ;
    skos:definition "Node in a 7x7 Risk Matrix with Risk Severity: Moderate; Likelihood: Moderate; and Risk Level: High"@en ;
    skos:prefLabel "High Risk (RM7x7 S:4 L:4)"@en .

risk-owl:RM7x7S4L5 a rdfs:Class,
        owl:Class,
        risk-owl:RiskAnalysis ;
    dct:contributor _:Ne22a67b17c7e4a779c30d2864b6a0cee ;
    dct:created "2022-08-17"^^xsd:date ;
    rdf:value "0.41,xsd:decimal" ;
    rdfs:isDefinedBy risk-owl: ;
    rdfs:subClassOf risk-owl:RiskMatrix7x7 ;
    sw:term_status "accepted"@en ;
    skos:definition "Node in a 7x7 Risk Matrix with Risk Severity: Moderate; Likelihood: High; and Risk Level: High"@en ;
    skos:prefLabel "High Risk (RM7x7 S:4 L:5)"@en .

risk-owl:RM7x7S4L6 a rdfs:Class,
        owl:Class,
        risk-owl:RiskAnalysis ;
    dct:contributor _:Ne22a67b17c7e4a779c30d2864b6a0cee ;
    dct:created "2022-08-17"^^xsd:date ;
    rdf:value "0.49,xsd:decimal" ;
    rdfs:isDefinedBy risk-owl: ;
    rdfs:subClassOf risk-owl:RiskMatrix7x7 ;
    sw:term_status "accepted"@en ;
    skos:definition "Node in a 7x7 Risk Matrix with Risk Severity: Moderate; Likelihood: Very High; and Risk Level: Very High"@en ;
    skos:prefLabel "Very High Risk (RM7x7 S:4 L:6)"@en .

risk-owl:RM7x7S4L7 a rdfs:Class,
        owl:Class,
        risk-owl:RiskAnalysis ;
    dct:contributor _:Ne22a67b17c7e4a779c30d2864b6a0cee ;
    dct:created "2022-08-17"^^xsd:date ;
    rdf:value "0.57,xsd:decimal" ;
    rdfs:isDefinedBy risk-owl: ;
    rdfs:subClassOf risk-owl:RiskMatrix7x7 ;
    sw:term_status "accepted"@en ;
    skos:definition "Node in a 7x7 Risk Matrix with Risk Severity: Moderate; Likelihood: Extremely High; and Risk Level: Very High"@en ;
    skos:prefLabel "Very High Risk (RM7x7 S:4 L:7)"@en .

risk-owl:RM7x7S5L1 a rdfs:Class,
        owl:Class,
        risk-owl:RiskAnalysis ;
    dct:contributor _:Ne22a67b17c7e4a779c30d2864b6a0cee ;
    dct:created "2022-08-17"^^xsd:date ;
    rdf:value "0.10,xsd:decimal" ;
    rdfs:isDefinedBy risk-owl: ;
    rdfs:subClassOf risk-owl:RiskMatrix7x7 ;
    sw:term_status "accepted"@en ;
    skos:definition "Node in a 7x7 Risk Matrix with Risk Severity: High; Likelihood: Extremely Low; and Risk Level: Very Low"@en ;
    skos:prefLabel "Very Low Risk (RM7x7 S:5 L:1)"@en .

risk-owl:RM7x7S5L2 a rdfs:Class,
        owl:Class,
        risk-owl:RiskAnalysis ;
    dct:contributor _:Ne22a67b17c7e4a779c30d2864b6a0cee ;
    dct:created "2022-08-17"^^xsd:date ;
    rdf:value "0.20,xsd:decimal" ;
    rdfs:isDefinedBy risk-owl: ;
    rdfs:subClassOf risk-owl:RiskMatrix7x7 ;
    sw:term_status "accepted"@en ;
    skos:definition "Node in a 7x7 Risk Matrix with Risk Severity: High; Likelihood: Very Low; and Risk Level: Low"@en ;
    skos:prefLabel "Low Risk (RM7x7 S:5 L:2)"@en .

risk-owl:RM7x7S5L3 a rdfs:Class,
        owl:Class,
        risk-owl:RiskAnalysis ;
    dct:contributor _:Ne22a67b17c7e4a779c30d2864b6a0cee ;
    dct:created "2022-08-17"^^xsd:date ;
    rdf:value "0.31,xsd:decimal" ;
    rdfs:isDefinedBy risk-owl: ;
    rdfs:subClassOf risk-owl:RiskMatrix7x7 ;
    sw:term_status "accepted"@en ;
    skos:definition "Node in a 7x7 Risk Matrix with Risk Severity: High; Likelihood: Low; and Risk Level: Moderate"@en ;
    skos:prefLabel "Moderate Risk (RM7x7 S:5 L:3)"@en .

risk-owl:RM7x7S5L4 a rdfs:Class,
        owl:Class,
        risk-owl:RiskAnalysis ;
    dct:contributor _:Ne22a67b17c7e4a779c30d2864b6a0cee ;
    dct:created "2022-08-17"^^xsd:date ;
    rdf:value "0.41,xsd:decimal" ;
    rdfs:isDefinedBy risk-owl: ;
    rdfs:subClassOf risk-owl:RiskMatrix7x7 ;
    sw:term_status "accepted"@en ;
    skos:definition "Node in a 7x7 Risk Matrix with Risk Severity: High; Likelihood: Moderate; and Risk Level: High"@en ;
    skos:prefLabel "High Risk (RM7x7 S:5 L:4)"@en .

risk-owl:RM7x7S5L5 a rdfs:Class,
        owl:Class,
        risk-owl:RiskAnalysis ;
    dct:contributor _:Ne22a67b17c7e4a779c30d2864b6a0cee ;
    dct:created "2022-08-17"^^xsd:date ;
    rdf:value "0.51,xsd:decimal" ;
    rdfs:isDefinedBy risk-owl: ;
    rdfs:subClassOf risk-owl:RiskMatrix7x7 ;
    sw:term_status "accepted"@en ;
    skos:definition "Node in a 7x7 Risk Matrix with Risk Severity: High; Likelihood: High; and Risk Level: Very High"@en ;
    skos:prefLabel "Very High Risk (RM7x7 S:5 L:5)"@en .

risk-owl:RM7x7S5L6 a rdfs:Class,
        owl:Class,
        risk-owl:RiskAnalysis ;
    dct:contributor _:Ne22a67b17c7e4a779c30d2864b6a0cee ;
    dct:created "2022-08-17"^^xsd:date ;
    rdf:value "0.61,xsd:decimal" ;
    rdfs:isDefinedBy risk-owl: ;
    rdfs:subClassOf risk-owl:RiskMatrix7x7 ;
    sw:term_status "accepted"@en ;
    skos:definition "Node in a 7x7 Risk Matrix with Risk Severity: High; Likelihood: Very High; and Risk Level: Extremely High"@en ;
    skos:prefLabel "Extremely High Risk (RM7x7 S:5 L:6)"@en .

risk-owl:RM7x7S5L7 a rdfs:Class,
        owl:Class,
        risk-owl:RiskAnalysis ;
    dct:contributor _:Ne22a67b17c7e4a779c30d2864b6a0cee ;
    dct:created "2022-08-17"^^xsd:date ;
    rdf:value "0.71,xsd:decimal" ;
    rdfs:isDefinedBy risk-owl: ;
    rdfs:subClassOf risk-owl:RiskMatrix7x7 ;
    sw:term_status "accepted"@en ;
    skos:definition "Node in a 7x7 Risk Matrix with Risk Severity: High; Likelihood: Extremely High; and Risk Level: Extremely High"@en ;
    skos:prefLabel "Extremely High Risk (RM7x7 S:5 L:7)"@en .

risk-owl:RM7x7S6L1 a rdfs:Class,
        owl:Class,
        risk-owl:RiskAnalysis ;
    dct:contributor _:Ne22a67b17c7e4a779c30d2864b6a0cee ;
    dct:created "2022-08-17"^^xsd:date ;
    rdf:value "0.12,xsd:decimal" ;
    rdfs:isDefinedBy risk-owl: ;
    rdfs:subClassOf risk-owl:RiskMatrix7x7 ;
    sw:term_status "accepted"@en ;
    skos:definition "Node in a 7x7 Risk Matrix with Risk Severity: Very High; Likelihood: Extremely Low; and Risk Level: Very Low"@en ;
    skos:prefLabel "Very Low Risk (RM7x7 S:6 L:1)"@en .

risk-owl:RM7x7S6L2 a rdfs:Class,
        owl:Class,
        risk-owl:RiskAnalysis ;
    dct:contributor _:Ne22a67b17c7e4a779c30d2864b6a0cee ;
    dct:created "2022-08-17"^^xsd:date ;
    rdf:value "0.24,xsd:decimal" ;
    rdfs:isDefinedBy risk-owl: ;
    rdfs:subClassOf risk-owl:RiskMatrix7x7 ;
    sw:term_status "accepted"@en ;
    skos:definition "Node in a 7x7 Risk Matrix with Risk Severity: Very High; Likelihood: Very Low; and Risk Level: Moderate"@en ;
    skos:prefLabel "Moderate Risk (RM7x7 S:6 L:2)"@en .

risk-owl:RM7x7S6L3 a rdfs:Class,
        owl:Class,
        risk-owl:RiskAnalysis ;
    dct:contributor _:Ne22a67b17c7e4a779c30d2864b6a0cee ;
    dct:created "2022-08-17"^^xsd:date ;
    rdf:value "0.37,xsd:decimal" ;
    rdfs:isDefinedBy risk-owl: ;
    rdfs:subClassOf risk-owl:RiskMatrix7x7 ;
    sw:term_status "accepted"@en ;
    skos:definition "Node in a 7x7 Risk Matrix with Risk Severity: Very High; Likelihood: Low; and Risk Level: High"@en ;
    skos:prefLabel "High Risk (RM7x7 S:6 L:3)"@en .

risk-owl:RM7x7S6L4 a rdfs:Class,
        owl:Class,
        risk-owl:RiskAnalysis ;
    dct:contributor _:Ne22a67b17c7e4a779c30d2864b6a0cee ;
    dct:created "2022-08-17"^^xsd:date ;
    rdf:value "0.49,xsd:decimal" ;
    rdfs:isDefinedBy risk-owl: ;
    rdfs:subClassOf risk-owl:RiskMatrix7x7 ;
    sw:term_status "accepted"@en ;
    skos:definition "Node in a 7x7 Risk Matrix with Risk Severity: Very High; Likelihood: Moderate; and Risk Level: Very High"@en ;
    skos:prefLabel "Very High Risk (RM7x7 S:6 L:4)"@en .

risk-owl:RM7x7S6L5 a rdfs:Class,
        owl:Class,
        risk-owl:RiskAnalysis ;
    dct:contributor _:Ne22a67b17c7e4a779c30d2864b6a0cee ;
    dct:created "2022-08-17"^^xsd:date ;
    rdf:value "0.61,xsd:decimal" ;
    rdfs:isDefinedBy risk-owl: ;
    rdfs:subClassOf risk-owl:RiskMatrix7x7 ;
    sw:term_status "accepted"@en ;
    skos:definition "Node in a 7x7 Risk Matrix with Risk Severity: Very High; Likelihood: High; and Risk Level: Very High"@en ;
    skos:prefLabel "Very High Risk (RM7x7 S:6 L:5)"@en .

risk-owl:RM7x7S6L6 a rdfs:Class,
        owl:Class,
        risk-owl:RiskAnalysis ;
    dct:contributor _:Ne22a67b17c7e4a779c30d2864b6a0cee ;
    dct:created "2022-08-17"^^xsd:date ;
    rdf:value "0.73,xsd:decimal" ;
    rdfs:isDefinedBy risk-owl: ;
    rdfs:subClassOf risk-owl:RiskMatrix7x7 ;
    sw:term_status "accepted"@en ;
    skos:definition "Node in a 7x7 Risk Matrix with Risk Severity: Very High; Likelihood: Very High; and Risk Level: Extremely High"@en ;
    skos:prefLabel "Extremely High Risk (RM7x7 S:6 L:6)"@en .

risk-owl:RM7x7S6L7 a rdfs:Class,
        owl:Class,
        risk-owl:RiskAnalysis ;
    dct:contributor _:Ne22a67b17c7e4a779c30d2864b6a0cee ;
    dct:created "2022-08-17"^^xsd:date ;
    rdf:value "0.86,xsd:decimal" ;
    rdfs:isDefinedBy risk-owl: ;
    rdfs:subClassOf risk-owl:RiskMatrix7x7 ;
    sw:term_status "accepted"@en ;
    skos:definition "Node in a 7x7 Risk Matrix with Risk Severity: Very High; Likelihood: Extremely High; and Risk Level: Extremely High"@en ;
    skos:prefLabel "Extremely High Risk (RM7x7 S:6 L:7)"@en .

risk-owl:RM7x7S7L1 a rdfs:Class,
        owl:Class,
        risk-owl:RiskAnalysis ;
    dct:contributor _:Ne22a67b17c7e4a779c30d2864b6a0cee ;
    dct:created "2022-08-17"^^xsd:date ;
    rdf:value "0.14,xsd:decimal" ;
    rdfs:isDefinedBy risk-owl: ;
    rdfs:subClassOf risk-owl:RiskMatrix7x7 ;
    sw:term_status "accepted"@en ;
    skos:definition "Node in a 7x7 Risk Matrix with Risk Severity: Extremely High; Likelihood: Extremely Low; and Risk Level: Low"@en ;
    skos:prefLabel "Low Risk (RM7x7 S:7 L:1)"@en .

risk-owl:RM7x7S7L2 a rdfs:Class,
        owl:Class,
        risk-owl:RiskAnalysis ;
    dct:contributor _:Ne22a67b17c7e4a779c30d2864b6a0cee ;
    dct:created "2022-08-17"^^xsd:date ;
    rdf:value "0.29,xsd:decimal" ;
    rdfs:isDefinedBy risk-owl: ;
    rdfs:subClassOf risk-owl:RiskMatrix7x7 ;
    sw:term_status "accepted"@en ;
    skos:definition "Node in a 7x7 Risk Matrix with Risk Severity: Extremely High; Likelihood: Very Low; and Risk Level: Moderate"@en ;
    skos:prefLabel "Moderate Risk (RM7x7 S:7 L:2)"@en .

risk-owl:RM7x7S7L3 a rdfs:Class,
        owl:Class,
        risk-owl:RiskAnalysis ;
    dct:contributor _:Ne22a67b17c7e4a779c30d2864b6a0cee ;
    dct:created "2022-08-17"^^xsd:date ;
    rdf:value "0.43,xsd:decimal" ;
    rdfs:isDefinedBy risk-owl: ;
    rdfs:subClassOf risk-owl:RiskMatrix7x7 ;
    sw:term_status "accepted"@en ;
    skos:definition "Node in a 7x7 Risk Matrix with Risk Severity: Extremely High; Likelihood: Low; and Risk Level: High"@en ;
    skos:prefLabel "High Risk (RM7x7 S:7 L:3)"@en .

risk-owl:RM7x7S7L4 a rdfs:Class,
        owl:Class,
        risk-owl:RiskAnalysis ;
    dct:contributor _:Ne22a67b17c7e4a779c30d2864b6a0cee ;
    dct:created "2022-08-17"^^xsd:date ;
    rdf:value "0.57,xsd:decimal" ;
    rdfs:isDefinedBy risk-owl: ;
    rdfs:subClassOf risk-owl:RiskMatrix7x7 ;
    sw:term_status "accepted"@en ;
    skos:definition "Node in a 7x7 Risk Matrix with Risk Severity: Extremely High; Likelihood: Moderate; and Risk Level: Very High"@en ;
    skos:prefLabel "Very High Risk (RM7x7 S:7 L:4)"@en .

risk-owl:RM7x7S7L5 a rdfs:Class,
        owl:Class,
        risk-owl:RiskAnalysis ;
    dct:contributor _:Ne22a67b17c7e4a779c30d2864b6a0cee ;
    dct:created "2022-08-17"^^xsd:date ;
    rdf:value "0.71,xsd:decimal" ;
    rdfs:isDefinedBy risk-owl: ;
    rdfs:subClassOf risk-owl:RiskMatrix7x7 ;
    sw:term_status "accepted"@en ;
    skos:definition "Node in a 7x7 Risk Matrix with Risk Severity: Extremely High; Likelihood: High; and Risk Level: Extremely High"@en ;
    skos:prefLabel "Extremely High Risk (RM7x7 S:7 L:5)"@en .

risk-owl:RM7x7S7L6 a rdfs:Class,
        owl:Class,
        risk-owl:RiskAnalysis ;
    dct:contributor _:Ne22a67b17c7e4a779c30d2864b6a0cee ;
    dct:created "2022-08-17"^^xsd:date ;
    rdf:value "0.86,xsd:decimal" ;
    rdfs:isDefinedBy risk-owl: ;
    rdfs:subClassOf risk-owl:RiskMatrix7x7 ;
    sw:term_status "accepted"@en ;
    skos:definition "Node in a 7x7 Risk Matrix with Risk Severity: Extremely High; Likelihood: Very High; and Risk Level: Extremely High"@en ;
    skos:prefLabel "Extremely High Risk (RM7x7 S:7 L:6)"@en .

risk-owl:RM7x7S7L7 a rdfs:Class,
        owl:Class,
        risk-owl:RiskAnalysis ;
    dct:contributor _:Ne22a67b17c7e4a779c30d2864b6a0cee ;
    dct:created "2022-08-17"^^xsd:date ;
    rdf:value "0.99,xsd:decimal" ;
    rdfs:isDefinedBy risk-owl: ;
    rdfs:subClassOf risk-owl:RiskMatrix7x7 ;
    sw:term_status "accepted"@en ;
    skos:definition "Node in a 7x7 Risk Matrix with Risk Severity: Extremely High; Likelihood: Extremely High; and Risk Level: Extremely High"@en ;
    skos:prefLabel "Extremely High Risk (RM7x7 S:7 L:7)"@en .

risk-owl:RacialDiscrimination a rdfs:Class,
        owl:Class,
        dpv-owl:RiskConcept,
        risk-owl:PotentialConsequence,
        risk-owl:PotentialImpact,
        risk-owl:PotentialRisk ;
    dct:created "2024-09-30"^^xsd:date ;
    rdfs:isDefinedBy risk-owl: ;
    rdfs:subClassOf risk-owl:Racism ;
    sw:term_status "accepted"@en ;
    skos:definition "Discrimination against individuals because of their racial background or skin color"@en ;
    skos:prefLabel "Racial Discrimination"@en .

risk-owl:Racism a rdfs:Class,
        owl:Class,
        dpv-owl:RiskConcept,
        risk-owl:PotentialConsequence,
        risk-owl:PotentialImpact,
        risk-owl:PotentialRisk ;
    dct:created "2024-09-30"^^xsd:date ;
    rdfs:isDefinedBy risk-owl: ;
    rdfs:subClassOf risk-owl:Discrimination ;
    sw:term_status "accepted"@en ;
    skos:definition "Prejudice or discrimination against people based on their race"@en ;
    skos:prefLabel "Racism"@en .

risk-owl:ReactiveControl a rdfs:Class,
        owl:Class,
        risk-owl:RiskControl ;
    dct:contributor _:Ne22a67b17c7e4a779c30d2864b6a0cee ;
    dct:created "2025-01-06"^^xsd:date ;
    rdfs:isDefinedBy risk-owl: ;
    rdfs:subClassOf risk-owl:RiskControl ;
    sw:term_status "accepted"@en ;
    skos:definition "Control that is established or functions after an event occurs"@en ;
    skos:prefLabel "Reactive Control"@en ;
    skos:scopeNote "The use of 'reactive' here refers to this control being established i.e. becoming active to address the effects of an event after they occur. It does not imply that the controls are put in place after the event or that there is no planned procedure for handling an incident"@en .

risk-owl:RecoveryControl a rdfs:Class,
        owl:Class,
        risk-owl:RiskControl ;
    dct:contributor _:N9c63c24625fe482386a350b4ea27b4f8,
        _:Ne22a67b17c7e4a779c30d2864b6a0cee ;
    dct:created "2024-05-19"^^xsd:date ;
    dct:modified "2025-01-06"^^xsd:date ;
    rdfs:isDefinedBy risk-owl: ;
    rdfs:subClassOf risk-owl:ResolutionControl ;
    sw:term_status "modified"@en ;
    skos:definition "Control that aims to restore the context following an event"@en ;
    skos:prefLabel "Recovery Control"@en ;
    skos:scopeNote "Recovery implies taking steps to correct the effects which may not be the same as the initial conditions before the event, whereas risk:ReversalControl refers to undoing the effects such that the initial condition is restored"@en .

risk-owl:ReduceLikelihood a rdfs:Class,
        owl:Class,
        risk-owl:RiskControl ;
    dct:contributor _:Ne22a67b17c7e4a779c30d2864b6a0cee ;
    dct:created "2024-05-19"^^xsd:date ;
    dct:modified "2025-01-06"^^xsd:date ;
    rdfs:isDefinedBy risk-owl: ;
    rdfs:subClassOf risk-owl:ReductionControl ;
    sw:term_status "modified"@en ;
    skos:definition "Control that reduces the likelihood of an event to occur"@en ;
    skos:prefLabel "Reduce Likelihood"@en .

risk-owl:ReduceSeverity a rdfs:Class,
        owl:Class,
        risk-owl:RiskControl ;
    dct:contributor _:Ne22a67b17c7e4a779c30d2864b6a0cee ;
    dct:created "2024-05-19"^^xsd:date ;
    dct:modified "2025-01-06"^^xsd:date ;
    rdfs:isDefinedBy risk-owl: ;
    rdfs:subClassOf risk-owl:ReductionControl ;
    sw:term_status "modified"@en ;
    skos:definition "Control that reduces the severity of an event's effects"@en ;
    skos:prefLabel "Reduce Severity"@en .

risk-owl:ReductionControl a rdfs:Class,
        owl:Class,
        risk-owl:RiskControl ;
    dct:created "2024-05-19"^^xsd:date ;
    dct:modified "2025-01-06"^^xsd:date ;
    rdfs:isDefinedBy risk-owl: ;
    rdfs:subClassOf risk-owl:ReactiveControl ;
    sw:term_status "modified"@en ;
    skos:definition "Control that reduces the effects of an event"@en ;
    skos:prefLabel "Reduction Control"@en ;
    skos:scopeNote "Reduction here refers to a lessening of the effects after the event has occured by either reducing their likelihood or their severity in the context. This can involve changing the underlying context such that the effects have a reduced chance of occuring, or to create additional measures such that the effects do not have the initial severity for an entity"@en .

risk-owl:Reidentification a rdfs:Class,
        owl:Class,
        dpv-owl:RiskConcept,
        risk-owl:ConfidentialityConcept,
        risk-owl:PotentialConsequence,
        risk-owl:PotentialRisk,
        risk-owl:PotentialRiskSource ;
    dct:contributor _:Ne22a67b17c7e4a779c30d2864b6a0cee ;
    dct:created "2022-08-19"^^xsd:date ;
    dct:modified "2024-08-16"^^xsd:date ;
    rdfs:isDefinedBy risk-owl: ;
    rdfs:subClassOf risk-owl:OperationalSecurityRisk ;
    sw:term_status "accepted"@en ;
    skos:definition "Concept representing Re-identification"@en ;
    skos:prefLabel "Re-identification"@en ;
    skos:scopeNote "Use this concept for reidentification in an internal context. For reidentification performed by external entities see concept UnauthorisedReidentification"@en .

risk-owl:ReligiousDiscrimination a rdfs:Class,
        owl:Class,
        dpv-owl:RiskConcept,
        risk-owl:PotentialConsequence,
        risk-owl:PotentialImpact,
        risk-owl:PotentialRisk ;
    dct:created "2024-09-30"^^xsd:date ;
    rdfs:isDefinedBy risk-owl: ;
    rdfs:subClassOf risk-owl:Discrimination ;
    sw:term_status "accepted"@en ;
    skos:definition "Discrimination based on a person's relligion or religious beliefs or practices"@en ;
    skos:prefLabel "Religious Discrimination"@en .

risk-owl:RemeditationControl a rdfs:Class,
        owl:Class,
        risk-owl:RiskControl ;
    dct:contributor _:N9c63c24625fe482386a350b4ea27b4f8,
        _:Ne22a67b17c7e4a779c30d2864b6a0cee ;
    dct:created "2024-05-19"^^xsd:date ;
    dct:modified "2025-01-06"^^xsd:date ;
    rdfs:isDefinedBy risk-owl: ;
    rdfs:subClassOf risk-owl:ResolutionControl ;
    sw:term_status "modified"@en ;
    skos:definition "Control that aims to fix or remedy the causes of an event to prevent further occurences"@en ;
    skos:prefLabel "Remeditation Control"@en ;
    skos:scopeNote "Remediation involves making changes in the context to avoid further events and effects, which may be for the specific event or for other similar events and effects. As such, remediation can also be undertaken as a proactive measure in the risk management lifecycle following an incident"@en .

risk-owl:RemoveConsequence a rdfs:Class,
        owl:Class,
        risk-owl:RiskControl ;
    dct:contributor _:Ne22a67b17c7e4a779c30d2864b6a0cee ;
    dct:created "2024-05-19"^^xsd:date ;
    dct:modified "2025-01-06"^^xsd:date ;
    rdfs:isDefinedBy risk-owl: ;
    rdfs:subClassOf risk-owl:ConsequenceControl,
        risk-owl:EliminationControl ;
    sw:term_status "modified"@en ;
    skos:definition "Control that proactively removes the consequence event such that the event does not occur in the context"@en ;
    skos:prefLabel "Remove Consequence"@en .

risk-owl:RemoveImpact a rdfs:Class,
        owl:Class,
        risk-owl:RiskControl ;
    dct:contributor _:Ne22a67b17c7e4a779c30d2864b6a0cee ;
    dct:created "2024-05-19"^^xsd:date ;
    dct:modified "2025-01-06"^^xsd:date ;
    rdfs:isDefinedBy risk-owl: ;
    rdfs:subClassOf risk-owl:EliminationControl,
        risk-owl:ImpactControl ;
    sw:term_status "modified"@en ;
    skos:definition "Control that proactively removes the impact event such that the event does not occur in the context"@en ;
    skos:prefLabel "Remove Impact"@en .

risk-owl:RemoveSource a rdfs:Class,
        owl:Class,
        risk-owl:RiskControl ;
    dct:contributor _:Ne22a67b17c7e4a779c30d2864b6a0cee ;
    dct:created "2024-05-19"^^xsd:date ;
    dct:modified "2025-01-06"^^xsd:date ;
    rdfs:isDefinedBy risk-owl: ;
    rdfs:subClassOf risk-owl:EliminationControl,
        risk-owl:SourceControl ;
    sw:term_status "modified"@en ;
    skos:definition "Control that proactively removes the risk source such that it is no longer present or applicable in the context"@en ;
    skos:prefLabel "Remove Source"@en .

risk-owl:Renumeration a rdfs:Class,
        owl:Class,
        dpv-owl:RiskConcept,
        risk-owl:PotentialConsequence,
        risk-owl:PotentialImpact,
        risk-owl:PotentialRisk ;
    dct:contributor _:N7d9b5ee7f31f4f2ba5951e30b49ec7c0,
        _:Ne22a67b17c7e4a779c30d2864b6a0cee ;
    dct:created "2024-04-14"^^xsd:date ;
    dct:modified "2024-08-16"^^xsd:date ;
    rdfs:isDefinedBy risk-owl: ;
    rdfs:subClassOf risk-owl:FinancialImpact ;
    sw:term_status "accepted"@en ;
    skos:definition "Something that acts as or provides renumeration which is in monetary or financial form"@en ;
    skos:prefLabel "Remuneration"@en .

risk-owl:ReputationalRisk a rdfs:Class,
        owl:Class,
        dpv-owl:RiskConcept,
        risk-owl:PotentialConsequence,
        risk-owl:PotentialImpact,
        risk-owl:PotentialRisk ;
    dct:created "2024-12-17"^^xsd:date ;
    rdfs:isDefinedBy risk-owl: ;
    rdfs:subClassOf risk-owl:OrganisationalRiskConcept ;
    sw:term_status "accepted"@en ;
    skos:definition "Risks and issues that affect the reputation of the organisation"@en ;
    skos:prefLabel "Reputational Risk"@en .

risk-owl:RequirementsBias a rdfs:Class,
        owl:Class,
        dpv-owl:RiskConcept,
        risk-owl:PotentialConsequence,
        risk-owl:PotentialRisk,
        risk-owl:PotentialRiskSource ;
    dct:contributor _:N2e9307242cb14d528effb994db501842,
        _:N9c63c24625fe482386a350b4ea27b4f8,
        _:Ne22a67b17c7e4a779c30d2864b6a0cee ;
    dct:created "2024-09-13"^^xsd:date ;
    dct:source "ISO/IEC 24027:2021"@en ;
    rdfs:isDefinedBy risk-owl: ;
    rdfs:subClassOf risk-owl:CognitiveBias ;
    sw:term_status "accepted"@en ;
    skos:definition "Bias that occurs in or during requirements creation"@en ;
    skos:prefLabel "Requirements Bias"@en ;
    skos:scopeNote "Requirements bias also represents occasions for the human cognitive biases to manifest"@en .

risk-owl:ResolutionControl a rdfs:Class,
        owl:Class,
        risk-owl:RiskControl ;
    dct:contributor _:Ne22a67b17c7e4a779c30d2864b6a0cee ;
    dct:created "2025-01-06"^^xsd:date ;
    rdfs:isDefinedBy risk-owl: ;
    rdfs:subClassOf risk-owl:ReactiveControl ;
    sw:term_status "accepted"@en ;
    skos:definition "Control that aims to resolve an event's effects with the goal of fixing or recovering from it"@en ;
    skos:prefLabel "Resolution Control"@en .

risk-owl:ReversalControl a rdfs:Class,
        owl:Class,
        risk-owl:RiskControl ;
    dct:contributor _:N9c63c24625fe482386a350b4ea27b4f8,
        _:Ne22a67b17c7e4a779c30d2864b6a0cee ;
    dct:created "2025-01-06"^^xsd:date ;
    rdfs:isDefinedBy risk-owl: ;
    rdfs:subClassOf risk-owl:ResolutionControl ;
    sw:term_status "accepted"@en ;
    skos:definition "Control that aims to reverse or undo the effects of an event"@en ;
    skos:prefLabel "Reversal Control"@en ;
    skos:scopeNote "Reversal can be achieved through measures such as restoring information from a backup or replacing things such that the initial context not containing the event's effects is restored"@en .

risk-owl:ReverseDiscrimination a rdfs:Class,
        owl:Class,
        dpv-owl:RiskConcept,
        risk-owl:PotentialConsequence,
        risk-owl:PotentialImpact,
        risk-owl:PotentialRisk ;
    dct:created "2024-09-30"^^xsd:date ;
    rdfs:isDefinedBy risk-owl: ;
    rdfs:subClassOf risk-owl:Discrimination ;
    sw:term_status "accepted"@en ;
    skos:definition "Discrimination against members of a majority or historically dominant group, often in the context of efforts to promote equality"@en ;
    skos:prefLabel "Reverse Discrimination"@en .

risk-owl:Reward a rdfs:Class,
        owl:Class,
        dpv-owl:RiskConcept,
        risk-owl:PotentialConsequence,
        risk-owl:PotentialImpact,
        risk-owl:PotentialRisk ;
    dct:contributor _:N7d9b5ee7f31f4f2ba5951e30b49ec7c0,
        _:Ne22a67b17c7e4a779c30d2864b6a0cee ;
    dct:created "2024-04-14"^^xsd:date ;
    dct:modified "2024-08-16"^^xsd:date ;
    rdfs:isDefinedBy risk-owl: ;
    rdfs:subClassOf risk-owl:Renumeration ;
    sw:term_status "accepted"@en ;
    skos:definition "Something that acts as or provides rewards i.e. a benefit given for some service or activity that is not a payment or fee"@en ;
    skos:prefLabel "Reward"@en .

risk-owl:RightsDenied a rdfs:Class,
        owl:Class,
        dpv-owl:RiskConcept,
        risk-owl:PotentialConsequence,
        risk-owl:PotentialImpact,
        risk-owl:PotentialRisk ;
    dct:created "2024-12-17"^^xsd:date ;
    rdfs:isDefinedBy risk-owl: ;
    rdfs:subClassOf risk-owl:RightsImpact ;
    sw:term_status "accepted"@en ;
    skos:definition "The refusal or withholding or denial of the existence or applicability of rights"@en ;
    skos:prefLabel "Rights Denied"@en ;
    skos:scopeNote "The denial of the right refers to the argument that a right does not apply at all for a particular case. Though specified as a plural i.e. 'rights', this concept can be applied to a singular right"@en .

risk-owl:RightsEroded a rdfs:Class,
        owl:Class,
        dpv-owl:RiskConcept,
        risk-owl:PotentialConsequence,
        risk-owl:PotentialImpact,
        risk-owl:PotentialRisk ;
    dct:created "2024-12-17"^^xsd:date ;
    rdfs:isDefinedBy risk-owl: ;
    rdfs:subClassOf risk-owl:RightsImpact ;
    sw:term_status "accepted"@en ;
    skos:definition "The gradual weakening or reduction of the scope and protection of rights"@en ;
    skos:prefLabel "Rights Eroded"@en ;
    skos:scopeNote "Erosion of rights typically only applies to passive rights which always apply, since for active rights the exercise of that    right is what enables it. An active right can be eroded over time it is limited consistently and increasingly such that the scope of the right is reduced over time. Though specified as a plural i.e. 'rights', this concept can be applied to a singular right"@en .

risk-owl:RightsExercisePrevented a rdfs:Class,
        owl:Class,
        dpv-owl:RiskConcept,
        risk-owl:PotentialConsequence,
        risk-owl:PotentialImpact,
        risk-owl:PotentialRisk ;
    dct:contributor _:N7d9b5ee7f31f4f2ba5951e30b49ec7c0,
        _:Ne22a67b17c7e4a779c30d2864b6a0cee ;
    dct:created "2022-08-18"^^xsd:date ;
    dct:modified "2024-08-16"^^xsd:date ;
    rdfs:isDefinedBy risk-owl: ;
    rdfs:subClassOf risk-owl:RightsImpact ;
    sw:term_status "accepted"@en ;
    skos:definition "Actions or measures that prevent an individual or group from exercising their legal rights."@en ;
    skos:prefLabel "Rights Exercise Prevented"@en ;
    skos:scopeNote "This concept was called \"PreventExercisingOfRights\" in DPV 2.0. Violation of a right is a bar for actionable actions by an authority. Other impacts on right may be found to construe a violation of the right, but that is not necessarily always the case i.e. not all impacts are violations of a right. Though specified as a plural i.e. 'rights', this concept can be applied to a singular right"@en .

risk-owl:RightsImpact a rdfs:Class,
        owl:Class,
        dpv-owl:RiskConcept,
        risk-owl:PotentialConsequence,
        risk-owl:PotentialImpact,
        risk-owl:PotentialRisk ;
    dct:contributor _:Ne22a67b17c7e4a779c30d2864b6a0cee ;
    dct:created "2022-08-17"^^xsd:date ;
    dct:modified "2024-08-16"^^xsd:date ;
    dct:source [ a schema:WebPage ;
            schema:name "ISO/IEC 27005:2018" ;
            schema:url "https://www.iso.org/standard/75281.html" ] ;
    vann:example dex-owl:E0088 ;
    rdfs:isDefinedBy risk-owl: ;
    rdfs:subClassOf risk-owl:SocietalRiskConcept ;
    sw:term_status "accepted"@en ;
    skos:definition "Concept representing Impact to Rights"@en ;
    skos:prefLabel "Rights Impact"@en ;
    skos:scopeNote "This concept was called \"ImpactToRights\" in DPV 2.0. Though specified as a plural i.e. 'rights', this concept can be applied to a singular right"@en .

risk-owl:RightsLimited a rdfs:Class,
        owl:Class,
        dpv-owl:RiskConcept,
        risk-owl:PotentialConsequence,
        risk-owl:PotentialImpact,
        risk-owl:PotentialRisk ;
    dct:contributor _:N7d9b5ee7f31f4f2ba5951e30b49ec7c0,
        _:Ne22a67b17c7e4a779c30d2864b6a0cee ;
    dct:created "2022-08-18"^^xsd:date ;
    dct:modified "2024-08-16"^^xsd:date ;
    rdfs:isDefinedBy risk-owl: ;
    rdfs:subClassOf risk-owl:RightsImpact ;
    sw:term_status "accepted"@en ;
    skos:definition "A limitation or restrictions on the scope or exercise of rights"@en ;
    skos:prefLabel "Rights Limited"@en ;
    skos:scopeNote "This concept was called \"LimitationOfRights\" in DPV 2.0. The    limitation refers to the applicability and scope of the right, and not in the ability to exercise that right. Limitation is therefore fulfilment of the right and its obligations - but for a scope other than what was intended or expected. Though specified as a plural i.e. 'rights', this concept can be applied to a singular right"@en .

risk-owl:RightsObstructed a rdfs:Class,
        owl:Class,
        dpv-owl:RiskConcept,
        risk-owl:PotentialConsequence,
        risk-owl:PotentialImpact,
        risk-owl:PotentialRisk ;
    dct:created "2024-12-17"^^xsd:date ;
    rdfs:isDefinedBy risk-owl: ;
    rdfs:subClassOf risk-owl:RightsImpact ;
    sw:term_status "accepted"@en ;
    skos:definition "Interference with or blocking of the exercise of rights"@en ;
    skos:prefLabel "Rights Obstructed"@en ;
    skos:scopeNote "In obstruction, the right is not denied, limited, or unfulfilled - but the requirements to enable exercise of the rights are increased to the point of discouraging or obstructing the exercise of that right. Though specified as a plural i.e. 'rights', this concept can be applied to a singular right"@en .

risk-owl:RightsUnfulfilled a rdfs:Class,
        owl:Class,
        dpv-owl:RiskConcept,
        risk-owl:PotentialConsequence,
        risk-owl:PotentialImpact,
        risk-owl:PotentialRisk ;
    dct:created "2024-12-17"^^xsd:date ;
    rdfs:isDefinedBy risk-owl: ;
    rdfs:subClassOf risk-owl:RightsImpact ;
    sw:term_status "accepted"@en ;
    skos:definition "Failure to meet or complete the fulfilment of rights"@en ;
    skos:prefLabel "Rights Unfulfilled"@en ;
    skos:scopeNote "Here unfulfilment refers to non-completion of the right's obligations and processes. Though specified as a plural i.e. 'rights', this concept can be applied to a singular right"@en .

risk-owl:RightsViolated a rdfs:Class,
        owl:Class,
        dpv-owl:RiskConcept,
        risk-owl:PotentialConsequence,
        risk-owl:PotentialImpact,
        risk-owl:PotentialRisk ;
    dct:contributor _:N7d9b5ee7f31f4f2ba5951e30b49ec7c0,
        _:Ne22a67b17c7e4a779c30d2864b6a0cee ;
    dct:created "2022-08-18"^^xsd:date ;
    dct:modified "2024-08-16"^^xsd:date ;
    vann:example dex-owl:E0088 ;
    rdfs:isDefinedBy risk-owl: ;
    rdfs:subClassOf risk-owl:RightsImpact ;
    sw:term_status "accepted"@en ;
    skos:definition "The infringement or breach of rights in a manner that constitutes a 'violation' of those rights"@en ;
    skos:prefLabel "Rights Violated"@en ;
    skos:scopeNote "This concept was called \"ViolationOfRights\" in DPV 2.0. Though specified as a plural i.e. 'rights', this concept can be applied to a singular right"@en .

risk-owl:RiskAcceptance a rdfs:Class,
        owl:Class ;
    dct:created "2024-12-01"^^xsd:date ;
    rdfs:isDefinedBy risk-owl: ;
    rdfs:subClassOf risk-owl:RiskManagement ;
    sw:term_status "accepted"@en ;
    skos:definition "Entity decision to accept or enable a particular risk"@en ;
    skos:prefLabel "Risk Acceptance"@en .

risk-owl:RiskAnalysis a rdfs:Class,
        owl:Class ;
    dct:contributor _:Ne22a67b17c7e4a779c30d2864b6a0cee ;
    dct:created "2022-08-18"^^xsd:date ;
    dct:source [ a schema:WebPage ;
            schema:name "IEC 31010:2019" ;
            schema:url "https://www.iso.org/standard/72140.html" ] ;
    rdfs:isDefinedBy risk-owl: ;
    rdfs:subClassOf risk-owl:RiskAssessment ;
    sw:term_status "accepted"@en ;
    skos:definition "A technique or method used to analyse and identify risk levels, sources, likelihoods, severities, and other necessary information required to conduct risk management procedures"@en ;
    skos:prefLabel "Risk Analysis"@en .

risk-owl:RiskAssessment a rdfs:Class,
        owl:Class ;
    dct:created "2024-02-14"^^xsd:date ;
    dct:source "ISO 31073:2022 Risk management vocabulary"@en ;
    rdfs:isDefinedBy risk-owl: ;
    rdfs:subClassOf risk-owl:RiskManagement ;
    sw:term_status "accepted"@en ;
    skos:definition "Assessment of risk involving its identification, analysis, and evaluation"@en ;
    skos:prefLabel "Risk Assessment"@en .

risk-owl:RiskControl a rdfs:Class,
        owl:Class ;
    dct:created "2024-05-19"^^xsd:date ;
    dct:modified "2025-01-06"^^xsd:date ;
    vann:example dex-owl:E0071,
        dex-owl:E0086 ;
    rdfs:isDefinedBy risk-owl: ;
    rdfs:subClassOf dpv-owl:RiskMitigationMeasure ;
    sw:term_status "accepted"@en ;
    skos:definition "Control that modifies risk"@en ;
    skos:prefLabel "Risk Control"@en .

risk-owl:RiskCriteria a rdfs:Class,
        owl:Class ;
    dct:created "2024-12-01"^^xsd:date ;
    rdfs:isDefinedBy risk-owl: ;
    rdfs:subClassOf risk-owl:RiskManagement ;
    sw:term_status "accepted"@en ;
    skos:definition "Criteria for determining or evaluating significance of risk"@en ;
    skos:prefLabel "Risk Criteria"@en .

risk-owl:RiskEvaluation a rdfs:Class,
        owl:Class ;
    dct:created "2024-12-01"^^xsd:date ;
    rdfs:isDefinedBy risk-owl: ;
    rdfs:subClassOf risk-owl:RiskAssessment ;
    sw:term_status "accepted"@en ;
    skos:definition "Process determining acceptability or tolerance of risk by comparing risk analysis outcomes against risk criteria"@en ;
    skos:prefLabel "Risk Evaluation"@en .

risk-owl:RiskIdentification a rdfs:Class,
        owl:Class ;
    dct:created "2024-12-01"^^xsd:date ;
    rdfs:isDefinedBy risk-owl: ;
    rdfs:subClassOf risk-owl:RiskAssessment ;
    sw:term_status "accepted"@en ;
    skos:definition "Identification of risks involving identification of risk sources, potential incidents, their causes, and their potential consequences"@en ;
    skos:prefLabel "Risk Identification"@en .

risk-owl:RiskManagement a rdfs:Class,
        owl:Class ;
    dct:created "2024-06-12"^^xsd:date ;
    dct:source "ISO 31073:2022 Risk management vocabulary"@en ;
    rdfs:isDefinedBy risk-owl: ;
    rdfs:subClassOf rdfs:Class ;
    sw:term_status "accepted"@en ;
    skos:definition "Systematic application of management policies, procedures, and practices for communicating, consulting, establishing context, and identifying, analysing, evaluating, treating, monitoring and reviewing risk. ISO 31000 definition: coordinated activities to direct and control an organization with regard to risk"@en ;
    skos:prefLabel "Risk Management"@en .

risk-owl:RiskMatrix a rdfs:Class,
        owl:Class ;
    dct:contributor _:Ne22a67b17c7e4a779c30d2864b6a0cee ;
    dct:created "2024-02-14"^^xsd:date ;
    dct:source [ a schema:WebPage ;
            schema:name "IEC 31010:2019" ;
            schema:url "https://www.iso.org/standard/72140.html" ] ;
    rdfs:isDefinedBy risk-owl: ;
    rdfs:subClassOf risk-owl:RiskAnalysis ;
    sw:term_status "accepted"@en ;
    skos:definition "Compares individual risks by selecting a consequence/ likelihood pair and displaying them on a matrix with consequence on one axis and likelihood on the other."@en ;
    skos:prefLabel "Risk Matrix"@en .

risk-owl:RiskMatrix3x3 a rdfs:Class,
        owl:Class,
        risk-owl:RiskAnalysis ;
    dct:contributor _:Ne22a67b17c7e4a779c30d2864b6a0cee ;
    dct:created "2022-08-17"^^xsd:date ;
    rdfs:isDefinedBy risk-owl: ;
    rdfs:subClassOf risk-owl:RiskMatrix ;
    sw:term_status "accepted"@en ;
    skos:definition "A Risk Matrix with 3 Likelihood, 3 Severity, and 3 Risk Level types"@en ;
    skos:prefLabel "Risk Matrix 3x3"@en .

risk-owl:RiskMatrix5x5 a rdfs:Class,
        owl:Class,
        risk-owl:RiskAnalysis ;
    dct:contributor _:Ne22a67b17c7e4a779c30d2864b6a0cee ;
    dct:created "2022-08-17"^^xsd:date ;
    rdfs:isDefinedBy risk-owl: ;
    rdfs:subClassOf risk-owl:RiskMatrix ;
    sw:term_status "accepted"@en ;
    skos:definition "A Risk Matrix with 5 Likelihood, 5 Severity, and 5 Risk Level types"@en ;
    skos:prefLabel "Risk Matrix 5x5"@en .

risk-owl:RiskMatrix7x7 a rdfs:Class,
        owl:Class,
        risk-owl:RiskAnalysis ;
    dct:contributor _:Ne22a67b17c7e4a779c30d2864b6a0cee ;
    dct:created "2022-08-17"^^xsd:date ;
    rdfs:isDefinedBy risk-owl: ;
    rdfs:subClassOf risk-owl:RiskMatrix ;
    sw:term_status "accepted"@en ;
    skos:definition "A Risk Matrix with 7 Likelihood, 7 Severity, and 7 Risk Level types"@en ;
    skos:prefLabel "Risk Matrix 7x7"@en .

risk-owl:RiskOwner a rdfs:Class,
        owl:Class ;
    dct:created "2024-12-01"^^xsd:date ;
    rdfs:isDefinedBy risk-owl: ;
    rdfs:subClassOf risk-owl:RiskManagement ;
    sw:term_status "accepted"@en ;
    skos:definition "Entity accountable for managing risk"@en ;
    skos:prefLabel "Risk Owner"@en .

risk-owl:RiskPerception a rdfs:Class,
        owl:Class ;
    dct:created "2024-12-01"^^xsd:date ;
    rdfs:isDefinedBy risk-owl: ;
    rdfs:subClassOf risk-owl:RiskManagement ;
    sw:term_status "accepted"@en ;
    skos:definition "Perception or view on risk"@en ;
    skos:prefLabel "Risk Perception"@en .

risk-owl:RiskSource a rdfs:Class,
        owl:Class ;
    dct:created "2024-02-14"^^xsd:date ;
    dct:modified "2024-08-16"^^xsd:date ;
    rdfs:isDefinedBy risk-owl: ;
    rdfs:subClassOf risk-owl:RiskIdentification ;
    sw:term_status "accepted"@en ;
    skos:definition "The 'cause' or 'source', which by itself or with another source has the potential to give rise to risk"@en ;
    skos:prefLabel "Risk Source"@en .

risk-owl:RiskTreatment a rdfs:Class,
        owl:Class ;
    dct:created "2024-12-01"^^xsd:date ;
    rdfs:isDefinedBy risk-owl: ;
    rdfs:subClassOf risk-owl:RiskManagement ;
    sw:term_status "accepted"@en ;
    skos:definition "Process by which risk is modified and mitigated"@en ;
    skos:prefLabel "Risk Treatment"@en .

risk-owl:RobustnessDegraded a rdfs:Class,
        owl:Class,
        dpv-owl:RiskConcept,
        risk-owl:PotentialConsequence,
        risk-owl:PotentialRisk,
        risk-owl:PotentialRiskSource ;
    dct:contributor _:N9c63c24625fe482386a350b4ea27b4f8,
        _:Ne22a67b17c7e4a779c30d2864b6a0cee ;
    dct:created "2024-12-01"^^xsd:date ;
    rdfs:isDefinedBy risk-owl: ;
    rdfs:subClassOf risk-owl:QualityDegraded,
        risk-owl:RobustnessRisk ;
    sw:term_status "accepted"@en ;
    skos:definition "Concepts representing risks and issues where Robustness is Degraded"@en ;
    skos:prefLabel "Robustness Degraded"@en .

risk-owl:RobustnessInconsistent a rdfs:Class,
        owl:Class,
        dpv-owl:RiskConcept,
        risk-owl:PotentialConsequence,
        risk-owl:PotentialRisk,
        risk-owl:PotentialRiskSource ;
    dct:contributor _:Ne22a67b17c7e4a779c30d2864b6a0cee ;
    dct:created "2024-12-01"^^xsd:date ;
    rdfs:isDefinedBy risk-owl: ;
    rdfs:subClassOf risk-owl:QualityInconsistent,
        risk-owl:RobustnessRisk ;
    sw:term_status "accepted"@en ;
    skos:definition "Concepts representing risks and issues where Robustness is Inconsistent"@en ;
    skos:prefLabel "Robustness Inconsistent"@en .

risk-owl:RobustnessInsufficient a rdfs:Class,
        owl:Class,
        dpv-owl:RiskConcept,
        risk-owl:PotentialConsequence,
        risk-owl:PotentialRisk,
        risk-owl:PotentialRiskSource ;
    dct:contributor _:N9c63c24625fe482386a350b4ea27b4f8,
        _:Ne22a67b17c7e4a779c30d2864b6a0cee ;
    dct:created "2024-12-01"^^xsd:date ;
    rdfs:isDefinedBy risk-owl: ;
    rdfs:subClassOf risk-owl:QualityInsufficient,
        risk-owl:RobustnessRisk ;
    sw:term_status "accepted"@en ;
    skos:definition "Concepts representing risks and issues where Robustness is Insufficient"@en ;
    skos:prefLabel "Robustness Insufficient"@en .

risk-owl:RobustnessRisk a rdfs:Class,
        owl:Class,
        dpv-owl:RiskConcept,
        risk-owl:PotentialConsequence,
        risk-owl:PotentialRisk,
        risk-owl:PotentialRiskSource ;
    dct:contributor _:Ne22a67b17c7e4a779c30d2864b6a0cee ;
    dct:created "2024-12-01"^^xsd:date ;
    rdfs:isDefinedBy risk-owl: ;
    rdfs:subClassOf risk-owl:QualityRisk ;
    sw:term_status "accepted"@en ;
    skos:definition "Concepts representing risks and issues where Robustness is Risk"@en ;
    skos:prefLabel "Robustness Risk"@en .

risk-owl:RobustnessUnknown a rdfs:Class,
        owl:Class,
        dpv-owl:RiskConcept,
        risk-owl:PotentialConsequence,
        risk-owl:PotentialRisk,
        risk-owl:PotentialRiskSource ;
    dct:contributor _:Ne22a67b17c7e4a779c30d2864b6a0cee ;
    dct:created "2024-12-01"^^xsd:date ;
    rdfs:isDefinedBy risk-owl: ;
    rdfs:subClassOf risk-owl:QualityUnknown,
        risk-owl:RobustnessRisk ;
    sw:term_status "accepted"@en ;
    skos:definition "Concepts representing risks and issues where Robustness is Unknown"@en ;
    skos:prefLabel "Robustness Unknown"@en .

risk-owl:RobustnessUnverified a rdfs:Class,
        owl:Class,
        dpv-owl:RiskConcept,
        risk-owl:PotentialConsequence,
        risk-owl:PotentialRisk,
        risk-owl:PotentialRiskSource ;
    dct:contributor _:Ne22a67b17c7e4a779c30d2864b6a0cee ;
    dct:created "2024-12-01"^^xsd:date ;
    rdfs:isDefinedBy risk-owl: ;
    rdfs:subClassOf risk-owl:QualityUnverified,
        risk-owl:RobustnessRisk ;
    sw:term_status "accepted"@en ;
    skos:definition "Concepts representing risks and issues where Robustness is Unverified"@en ;
    skos:prefLabel "Robustness Unverified"@en .

risk-owl:RuleBasedSystemDesign a rdfs:Class,
        owl:Class,
        dpv-owl:RiskConcept,
        risk-owl:PotentialConsequence,
        risk-owl:PotentialRisk,
        risk-owl:PotentialRiskSource ;
    dct:contributor _:N2e9307242cb14d528effb994db501842,
        _:N9c63c24625fe482386a350b4ea27b4f8,
        _:Ne22a67b17c7e4a779c30d2864b6a0cee ;
    dct:created "2024-09-13"^^xsd:date ;
    dct:source "ISO/IEC 24027:2021"@en ;
    rdfs:isDefinedBy risk-owl: ;
    rdfs:subClassOf risk-owl:CognitiveBias ;
    sw:term_status "accepted"@en ;
    skos:definition "Bias that occurs due to developer experience and expert advice having a significant influence on rule-based system design"@en ;
    skos:prefLabel "Rule-Based System Design"@en ;
    skos:scopeNote "Rule based system design also potentially introduces various forms of human cognitive bias"@en .

risk-owl:Sabotage a rdfs:Class,
        owl:Class,
        dpv-owl:RiskConcept,
        risk-owl:AvailabilityConcept,
        risk-owl:IntegrityConcept,
        risk-owl:PotentialConsequence,
        risk-owl:PotentialRisk,
        risk-owl:PotentialRiskSource ;
    dct:contributor _:Ne22a67b17c7e4a779c30d2864b6a0cee ;
    dct:created "2022-08-17"^^xsd:date ;
    dct:modified "2024-08-16"^^xsd:date ;
    dct:source [ a schema:WebPage ;
            schema:name "ENISA Reference Incident Classification Taxonomy 2018" ;
            schema:url "https://www.enisa.europa.eu/publications/reference-incident-classification-taxonomy/" ] ;
    rdfs:isDefinedBy risk-owl: ;
    rdfs:subClassOf risk-owl:MaliciousActivity ;
    sw:term_status "accepted"@en ;
    skos:definition "Concept representing Sabotage"@en ;
    skos:prefLabel "Sabotage"@en .

risk-owl:Safety a rdfs:Class,
        owl:Class,
        dpv-owl:RiskConcept,
        risk-owl:PotentialConsequence,
        risk-owl:PotentialImpact,
        risk-owl:PotentialRisk ;
    dct:contributor _:Ne22a67b17c7e4a779c30d2864b6a0cee ;
    dct:created "2024-12-01"^^xsd:date ;
    rdfs:isDefinedBy risk-owl: ;
    rdfs:subClassOf risk-owl:HealthSafety ;
    sw:term_status "accepted"@en ;
    skos:definition "Concept representing safety of individual(s), or group(s), or society at large"@en ;
    skos:prefLabel "Safety"@en .

risk-owl:SamplingBias a rdfs:Class,
        owl:Class,
        dpv-owl:RiskConcept,
        risk-owl:PotentialConsequence,
        risk-owl:PotentialRisk,
        risk-owl:PotentialRiskSource ;
    dct:contributor _:N2e9307242cb14d528effb994db501842,
        _:N9c63c24625fe482386a350b4ea27b4f8,
        _:Ne22a67b17c7e4a779c30d2864b6a0cee ;
    dct:created "2024-09-13"^^xsd:date ;
    dct:source "ISO/IEC 24027:2021"@en ;
    rdfs:isDefinedBy risk-owl: ;
    rdfs:subClassOf risk-owl:SelectionBias ;
    sw:term_status "accepted"@en ;
    skos:definition "Bias that occurs when data records are not collected randomly from the intended population"@en ;
    skos:prefLabel "Sampling Bias"@en .

risk-owl:Scam a rdfs:Class,
        owl:Class,
        dpv-owl:RiskConcept,
        risk-owl:ConfidentialityConcept,
        risk-owl:PotentialConsequence,
        risk-owl:PotentialRisk,
        risk-owl:PotentialRiskSource ;
    dct:contributor _:Ne22a67b17c7e4a779c30d2864b6a0cee ;
    dct:created "2022-08-17"^^xsd:date ;
    dct:modified "2024-08-16"^^xsd:date ;
    dct:source [ a schema:WebPage ;
            schema:name "ISO/IEC 27005:2018" ;
            schema:url "https://www.iso.org/standard/75281.html" ] ;
    rdfs:isDefinedBy risk-owl: ;
    rdfs:subClassOf risk-owl:MaliciousActivity ;
    sw:term_status "accepted"@en ;
    skos:definition "Concept representing Scam"@en ;
    skos:prefLabel "Scam"@en .

risk-owl:SecurityAttack a rdfs:Class,
        owl:Class,
        dpv-owl:RiskConcept,
        risk-owl:AvailabilityConcept,
        risk-owl:ConfidentialityConcept,
        risk-owl:IntegrityConcept,
        risk-owl:PotentialRisk,
        risk-owl:PotentialRiskSource ;
    dct:created "2024-12-17"^^xsd:date ;
    rdfs:isDefinedBy risk-owl: ;
    rdfs:subClassOf risk-owl:ExternalSecurityThreat ;
    sw:term_status "accepted"@en ;
    skos:definition "Concept representing an attack on security with the aim of undermining it"@en ;
    skos:prefLabel "Security Attack"@en .

risk-owl:SecurityBreach a rdfs:Class,
        owl:Class,
        dpv-owl:RiskConcept,
        risk-owl:AvailabilityConcept,
        risk-owl:ConfidentialityConcept,
        risk-owl:IntegrityConcept,
        risk-owl:PotentialConsequence,
        risk-owl:PotentialRisk,
        risk-owl:PotentialRiskSource ;
    dct:contributor _:Ne22a67b17c7e4a779c30d2864b6a0cee ;
    dct:created "2022-08-17"^^xsd:date ;
    dct:modified "2024-08-16"^^xsd:date ;
    dct:source [ a schema:WebPage ;
            schema:name "ISO/IEC 27005:2018" ;
            schema:url "https://www.iso.org/standard/75281.html" ] ;
    rdfs:isDefinedBy risk-owl: ;
    rdfs:subClassOf risk-owl:OperationalSecurityRisk ;
    sw:term_status "accepted"@en ;
    skos:definition "Concept representing Security Breach"@en ;
    skos:prefLabel "Security Breach"@en .

risk-owl:SecurityQualityDegraded a rdfs:Class,
        owl:Class,
        dpv-owl:RiskConcept,
        risk-owl:PotentialConsequence,
        risk-owl:PotentialRisk,
        risk-owl:PotentialRiskSource ;
    dct:contributor _:N9c63c24625fe482386a350b4ea27b4f8,
        _:Ne22a67b17c7e4a779c30d2864b6a0cee ;
    dct:created "2024-12-01"^^xsd:date ;
    rdfs:isDefinedBy risk-owl: ;
    rdfs:subClassOf risk-owl:QualityDegraded,
        risk-owl:SecurityQualityRisk ;
    sw:term_status "accepted"@en ;
    skos:definition "Concepts representing risks and issues where Quality of Security is Degraded"@en ;
    skos:prefLabel "Security Quality Degraded"@en .

risk-owl:SecurityQualityInconsistent a rdfs:Class,
        owl:Class,
        dpv-owl:RiskConcept,
        risk-owl:PotentialConsequence,
        risk-owl:PotentialRisk,
        risk-owl:PotentialRiskSource ;
    dct:contributor _:Ne22a67b17c7e4a779c30d2864b6a0cee ;
    dct:created "2024-12-01"^^xsd:date ;
    rdfs:isDefinedBy risk-owl: ;
    rdfs:subClassOf risk-owl:QualityInconsistent,
        risk-owl:SecurityQualityRisk ;
    sw:term_status "accepted"@en ;
    skos:definition "Concepts representing risks and issues where Quality of Security is Inconsistent"@en ;
    skos:prefLabel "Security Quality Inconsistent"@en .

risk-owl:SecurityQualityInsufficient a rdfs:Class,
        owl:Class,
        dpv-owl:RiskConcept,
        risk-owl:PotentialConsequence,
        risk-owl:PotentialRisk,
        risk-owl:PotentialRiskSource ;
    dct:contributor _:N9c63c24625fe482386a350b4ea27b4f8,
        _:Ne22a67b17c7e4a779c30d2864b6a0cee ;
    dct:created "2024-12-01"^^xsd:date ;
    rdfs:isDefinedBy risk-owl: ;
    rdfs:subClassOf risk-owl:QualityInsufficient,
        risk-owl:SecurityQualityRisk ;
    sw:term_status "accepted"@en ;
    skos:definition "Concepts representing risks and issues where Quality of Security is Insufficient"@en ;
    skos:prefLabel "Security Quality Insufficient"@en .

risk-owl:SecurityQualityRisk a rdfs:Class,
        owl:Class,
        dpv-owl:RiskConcept,
        risk-owl:PotentialConsequence,
        risk-owl:PotentialRisk,
        risk-owl:PotentialRiskSource ;
    dct:contributor _:Ne22a67b17c7e4a779c30d2864b6a0cee ;
    dct:created "2024-12-01"^^xsd:date ;
    rdfs:isDefinedBy risk-owl: ;
    rdfs:subClassOf risk-owl:QualityRisk ;
    sw:term_status "accepted"@en ;
    skos:definition "Concepts representing risks and issues where Quality of Security is Risk"@en ;
    skos:prefLabel "Security Quality Risk"@en .

risk-owl:SecurityQualityUnknown a rdfs:Class,
        owl:Class,
        dpv-owl:RiskConcept,
        risk-owl:PotentialConsequence,
        risk-owl:PotentialRisk,
        risk-owl:PotentialRiskSource ;
    dct:contributor _:Ne22a67b17c7e4a779c30d2864b6a0cee ;
    dct:created "2024-12-01"^^xsd:date ;
    rdfs:isDefinedBy risk-owl: ;
    rdfs:subClassOf risk-owl:QualityUnknown,
        risk-owl:SecurityQualityRisk ;
    sw:term_status "accepted"@en ;
    skos:definition "Concepts representing risks and issues where Quality of Security is Unknown"@en ;
    skos:prefLabel "Security Quality Unknown"@en .

risk-owl:SecurityQualityUnverified a rdfs:Class,
        owl:Class,
        dpv-owl:RiskConcept,
        risk-owl:PotentialConsequence,
        risk-owl:PotentialRisk,
        risk-owl:PotentialRiskSource ;
    dct:contributor _:Ne22a67b17c7e4a779c30d2864b6a0cee ;
    dct:created "2024-12-01"^^xsd:date ;
    rdfs:isDefinedBy risk-owl: ;
    rdfs:subClassOf risk-owl:QualityUnverified,
        risk-owl:SecurityQualityRisk ;
    sw:term_status "accepted"@en ;
    skos:definition "Concepts representing risks and issues where Quality of Security is Unverified"@en ;
    skos:prefLabel "Security Quality Unverified"@en .

risk-owl:SelectionBias a rdfs:Class,
        owl:Class,
        dpv-owl:RiskConcept,
        risk-owl:PotentialConsequence,
        risk-owl:PotentialRisk,
        risk-owl:PotentialRiskSource ;
    dct:contributor _:N2e9307242cb14d528effb994db501842,
        _:N9c63c24625fe482386a350b4ea27b4f8,
        _:Ne22a67b17c7e4a779c30d2864b6a0cee ;
    dct:created "2024-09-13"^^xsd:date ;
    dct:source "ISO/IEC 24027:2021"@en ;
    rdfs:isDefinedBy risk-owl: ;
    rdfs:subClassOf risk-owl:StatisticalBias ;
    sw:term_status "accepted"@en ;
    skos:definition "Bias that occurs when a dataset's samples are chosen in a way that is not reflective of their real-world distribution"@en ;
    skos:prefLabel "Selection Bias"@en .

risk-owl:ServiceAlternativeOffered a rdfs:Class,
        owl:Class,
        dpv-owl:RiskConcept,
        risk-owl:PotentialConsequence,
        risk-owl:PotentialImpact,
        risk-owl:PotentialRisk ;
    dct:created "2024-10-21"^^xsd:date ;
    rdfs:isDefinedBy risk-owl: ;
    rdfs:subClassOf risk-owl:ServiceRelatedConsequence ;
    sw:term_status "accepted"@en ;
    skos:definition "Concept representing service alternative offered"@en ;
    skos:prefLabel "Service Alternative Offered"@en .

risk-owl:ServiceCostIncreased a rdfs:Class,
        owl:Class,
        dpv-owl:RiskConcept,
        risk-owl:PotentialConsequence,
        risk-owl:PotentialImpact,
        risk-owl:PotentialRisk ;
    dct:created "2024-10-21"^^xsd:date ;
    rdfs:isDefinedBy risk-owl: ;
    rdfs:subClassOf risk-owl:ServiceRelatedConsequence ;
    sw:term_status "accepted"@en ;
    skos:definition "Concept representing service cost increased"@en ;
    skos:prefLabel "Service Cost Increased"@en .

risk-owl:ServiceDenied a rdfs:Class,
        owl:Class,
        dpv-owl:RiskConcept,
        risk-owl:PotentialConsequence,
        risk-owl:PotentialImpact,
        risk-owl:PotentialRisk ;
    dct:created "2024-10-21"^^xsd:date ;
    rdfs:isDefinedBy risk-owl: ;
    rdfs:subClassOf risk-owl:ServiceRelatedConsequence ;
    sw:term_status "accepted"@en ;
    skos:definition "Concept representing service denied"@en ;
    skos:prefLabel "Service Denied"@en .

risk-owl:ServiceLimited a rdfs:Class,
        owl:Class,
        dpv-owl:RiskConcept,
        risk-owl:PotentialConsequence,
        risk-owl:PotentialImpact,
        risk-owl:PotentialRisk ;
    dct:created "2024-10-21"^^xsd:date ;
    rdfs:isDefinedBy risk-owl: ;
    rdfs:subClassOf risk-owl:ServiceRelatedConsequence ;
    sw:term_status "accepted"@en ;
    skos:definition "Concept representing service limited"@en ;
    skos:prefLabel "Service Limited"@en .

risk-owl:ServiceNotProvided a rdfs:Class,
        owl:Class,
        dpv-owl:RiskConcept,
        risk-owl:PotentialConsequence,
        risk-owl:PotentialImpact,
        risk-owl:PotentialRisk ;
    dct:created "2024-10-21"^^xsd:date ;
    rdfs:isDefinedBy risk-owl: ;
    rdfs:subClassOf risk-owl:ServiceRelatedConsequence ;
    sw:term_status "accepted"@en ;
    skos:definition "Concept representing service not provided"@en ;
    skos:prefLabel "Service Not Provided"@en .

risk-owl:ServicePartiallyProvided a rdfs:Class,
        owl:Class,
        dpv-owl:RiskConcept,
        risk-owl:PotentialConsequence,
        risk-owl:PotentialImpact,
        risk-owl:PotentialRisk ;
    dct:created "2024-10-21"^^xsd:date ;
    rdfs:isDefinedBy risk-owl: ;
    rdfs:subClassOf risk-owl:ServiceRelatedConsequence ;
    sw:term_status "accepted"@en ;
    skos:definition "Concept representing service partially provided"@en ;
    skos:prefLabel "Service Partially Provided"@en .

risk-owl:ServiceProvided a rdfs:Class,
        owl:Class,
        dpv-owl:RiskConcept,
        risk-owl:PotentialConsequence,
        risk-owl:PotentialImpact,
        risk-owl:PotentialRisk ;
    dct:created "2024-10-21"^^xsd:date ;
    rdfs:isDefinedBy risk-owl: ;
    rdfs:subClassOf risk-owl:ServiceRelatedConsequence ;
    sw:term_status "accepted"@en ;
    skos:definition "Concept representing service provided"@en ;
    skos:prefLabel "Service Provided"@en .

risk-owl:ServiceProvisionDelayed a rdfs:Class,
        owl:Class,
        dpv-owl:RiskConcept,
        risk-owl:PotentialConsequence,
        risk-owl:PotentialImpact,
        risk-owl:PotentialRisk ;
    dct:created "2024-10-21"^^xsd:date ;
    rdfs:isDefinedBy risk-owl: ;
    rdfs:subClassOf risk-owl:ServiceRelatedConsequence ;
    sw:term_status "accepted"@en ;
    skos:definition "Concept representing service provision delayed"@en ;
    skos:prefLabel "Service Provision Delayed"@en .

risk-owl:ServiceQualityReduced a rdfs:Class,
        owl:Class,
        dpv-owl:RiskConcept,
        risk-owl:PotentialConsequence,
        risk-owl:PotentialImpact,
        risk-owl:PotentialRisk ;
    dct:created "2024-10-21"^^xsd:date ;
    rdfs:isDefinedBy risk-owl: ;
    rdfs:subClassOf risk-owl:ServiceRelatedConsequence ;
    sw:term_status "accepted"@en ;
    skos:definition "Concept representing service quality reduced"@en ;
    skos:prefLabel "Service Quality Reduced"@en .

risk-owl:ServiceRelatedConsequence a rdfs:Class,
        owl:Class,
        dpv-owl:RiskConcept,
        risk-owl:PotentialConsequence,
        risk-owl:PotentialImpact,
        risk-owl:PotentialRisk ;
    dct:created "2024-10-21"^^xsd:date ;
    rdfs:isDefinedBy risk-owl: ;
    rdfs:subClassOf risk-owl:OrganisationalRiskConcept ;
    sw:term_status "accepted"@en ;
    skos:definition "A consequence related to the provision of a service"@en ;
    skos:prefLabel "Service Related Consequence"@en .

risk-owl:ServiceSecurityReduced a rdfs:Class,
        owl:Class,
        dpv-owl:RiskConcept,
        risk-owl:PotentialConsequence,
        risk-owl:PotentialImpact,
        risk-owl:PotentialRisk ;
    dct:created "2024-10-21"^^xsd:date ;
    rdfs:isDefinedBy risk-owl: ;
    rdfs:subClassOf risk-owl:ServiceRelatedConsequence ;
    sw:term_status "accepted"@en ;
    skos:definition "Concept representing service security reduced"@en ;
    skos:prefLabel "Service Security Reduced"@en .

risk-owl:ServiceTermination a rdfs:Class,
        owl:Class,
        dpv-owl:RiskConcept,
        risk-owl:PotentialConsequence,
        risk-owl:PotentialImpact,
        risk-owl:PotentialRisk ;
    dct:created "2024-10-21"^^xsd:date ;
    rdfs:isDefinedBy risk-owl: ;
    rdfs:subClassOf risk-owl:ServiceRelatedConsequence ;
    sw:term_status "accepted"@en ;
    skos:definition "Concept representing service termination"@en ;
    skos:prefLabel "Service Termination"@en .

risk-owl:SexDiscrimination a rdfs:Class,
        owl:Class,
        dpv-owl:RiskConcept,
        risk-owl:PotentialConsequence,
        risk-owl:PotentialImpact,
        risk-owl:PotentialRisk ;
    dct:created "2024-09-30"^^xsd:date ;
    rdfs:isDefinedBy risk-owl: ;
    rdfs:subClassOf risk-owl:Sexism ;
    sw:term_status "accepted"@en ;
    skos:definition "Discrimination based on a person's biological sex"@en ;
    skos:prefLabel "Sex Discrimination"@en .

risk-owl:Sexism a rdfs:Class,
        owl:Class,
        dpv-owl:RiskConcept,
        risk-owl:PotentialConsequence,
        risk-owl:PotentialImpact,
        risk-owl:PotentialRisk ;
    dct:created "2024-09-30"^^xsd:date ;
    rdfs:isDefinedBy risk-owl: ;
    rdfs:subClassOf risk-owl:Discrimination ;
    sw:term_status "accepted"@en ;
    skos:definition "Discrimination based on a person's sex or gender, typically involving unequal treatment or stereotyping"@en ;
    skos:prefLabel "Sexism"@en .

risk-owl:SexualHarassment a rdfs:Class,
        owl:Class,
        dpv-owl:RiskConcept,
        risk-owl:PotentialConsequence,
        risk-owl:PotentialImpact,
        risk-owl:PotentialRisk ;
    dct:created "2022-08-17"^^xsd:date ;
    dct:modified "2024-12-01"^^xsd:date ;
    rdfs:isDefinedBy risk-owl: ;
    rdfs:subClassOf risk-owl:Harassment ;
    sw:term_status "modified"@en ;
    skos:definition "Concept representing sexual harassment of individual(s)"@en ;
    skos:prefLabel "Sexual Harassment"@en .

risk-owl:SexualOrientationDiscrimination a rdfs:Class,
        owl:Class,
        dpv-owl:RiskConcept,
        risk-owl:PotentialConsequence,
        risk-owl:PotentialImpact,
        risk-owl:PotentialRisk ;
    dct:created "2024-09-30"^^xsd:date ;
    rdfs:isDefinedBy risk-owl: ;
    rdfs:subClassOf risk-owl:Discrimination ;
    sw:term_status "accepted"@en ;
    skos:definition "Discrimination based on a person's sexual orientation, typically against those who are not heterosexual"@en ;
    skos:prefLabel "SexualOrientation Discrimination"@en .

risk-owl:SexualViolence a rdfs:Class,
        owl:Class,
        dpv-owl:RiskConcept,
        risk-owl:PotentialConsequence,
        risk-owl:PotentialImpact,
        risk-owl:PotentialRisk ;
    dct:contributor _:Ne22a67b17c7e4a779c30d2864b6a0cee ;
    dct:created "2022-08-17"^^xsd:date ;
    dct:modified "2024-08-16"^^xsd:date ;
    dct:source [ a schema:WebPage ;
            schema:name "ENISA Reference Incident Classification Taxonomy 2018" ;
            schema:url "https://www.enisa.europa.eu/publications/reference-incident-classification-taxonomy/" ] ;
    rdfs:isDefinedBy risk-owl: ;
    rdfs:subClassOf risk-owl:Harm,
        risk-owl:MentalSafety,
        risk-owl:PhysicalSafety ;
    sw:term_status "accepted"@en ;
    skos:definition "Concept representing Sexual Violence"@en ;
    skos:prefLabel "Sexual Violence"@en .

risk-owl:ShareControl a rdfs:Class,
        owl:Class,
        risk-owl:RiskControl ;
    dct:contributor _:Ne22a67b17c7e4a779c30d2864b6a0cee ;
    dct:created "2025-01-06"^^xsd:date ;
    rdfs:isDefinedBy risk-owl: ;
    rdfs:subClassOf risk-owl:TransferControl ;
    sw:term_status "accepted"@en ;
    skos:definition "Control that aims to share or distribute the event (or risk) with another context or entity"@en ;
    skos:prefLabel "Share Control"@en ;
    skos:scopeNote "Sharing implies a combined responsibility or sharing of effects from an event - which can be between entities or procesess (or other contexts). The use of 'event' here broadly refers to any event, which may be a risk event or could also be specific measures being adopted in response to an event. For specifically indicating sharing of risk per typical risk management processes, see risk:ShareRisk"@en .

risk-owl:ShareRisk a rdfs:Class,
        owl:Class,
        risk-owl:RiskControl ;
    dct:contributor _:Ne22a67b17c7e4a779c30d2864b6a0cee ;
    dct:created "2024-05-19"^^xsd:date ;
    dct:modified "2025-01-06"^^xsd:date ;
    rdfs:isDefinedBy risk-owl: ;
    rdfs:subClassOf risk-owl:ShareControl ;
    sw:term_status "modified"@en ;
    skos:definition "Risk Mitigation Measure that shares Risk e.g. amongst stakeholders"@en ;
    skos:prefLabel "Share Risk"@en .

risk-owl:SimpsonsParadoxBias a rdfs:Class,
        owl:Class,
        dpv-owl:RiskConcept,
        risk-owl:PotentialConsequence,
        risk-owl:PotentialRisk,
        risk-owl:PotentialRiskSource ;
    dct:contributor _:N2e9307242cb14d528effb994db501842,
        _:N9c63c24625fe482386a350b4ea27b4f8,
        _:Ne22a67b17c7e4a779c30d2864b6a0cee ;
    dct:created "2024-09-13"^^xsd:date ;
    dct:source "ISO/IEC 24027:2021"@en ;
    rdfs:isDefinedBy risk-owl: ;
    rdfs:subClassOf risk-owl:DataBias ;
    sw:term_status "accepted"@en ;
    skos:definition "Bias that occurs when a trend that is indicated in individual groups of data reverses when the groups of data are combined"@en ;
    skos:prefLabel "Simpson'S Paradox Bias"@en .

risk-owl:SocialDisadvantage a rdfs:Class,
        owl:Class,
        dpv-owl:RiskConcept,
        risk-owl:PotentialConsequence,
        risk-owl:PotentialImpact,
        risk-owl:PotentialRisk ;
    dct:contributor _:N7d9b5ee7f31f4f2ba5951e30b49ec7c0 ;
    dct:created "2022-08-19"^^xsd:date ;
    dct:modified "2024-08-16"^^xsd:date ;
    rdfs:isDefinedBy risk-owl: ;
    rdfs:subClassOf risk-owl:GroupRisk ;
    sw:term_status "accepted"@en ;
    skos:definition "Concept representing Social Disadvantage"@en ;
    skos:prefLabel "Social Disadvantage"@en .

risk-owl:SocietalBias a rdfs:Class,
        owl:Class,
        dpv-owl:RiskConcept,
        risk-owl:PotentialConsequence,
        risk-owl:PotentialRisk,
        risk-owl:PotentialRiskSource ;
    dct:contributor _:N2e9307242cb14d528effb994db501842,
        _:N9c63c24625fe482386a350b4ea27b4f8,
        _:Ne22a67b17c7e4a779c30d2864b6a0cee ;
    dct:created "2024-09-13"^^xsd:date ;
    dct:source "ISO/IEC 24027:2021"@en ;
    rdfs:isDefinedBy risk-owl: ;
    rdfs:subClassOf risk-owl:CognitiveBias ;
    sw:term_status "accepted"@en ;
    skos:definition "Bias that occurs when similiar cognitive bias (conscious or unconscious) is being held by many individuals in society"@en ;
    skos:prefLabel "Societal Bias"@en .

risk-owl:SocietalHealthSafety a rdfs:Class,
        owl:Class,
        dpv-owl:RiskConcept,
        risk-owl:PotentialConsequence,
        risk-owl:PotentialImpact,
        risk-owl:PotentialRisk ;
    dct:created "2024-12-17"^^xsd:date ;
    rdfs:isDefinedBy risk-owl: ;
    rdfs:subClassOf risk-owl:GroupRisk ;
    sw:term_status "accepted"@en ;
    skos:definition "Concept representing health and safety of society at large"@en ;
    skos:prefLabel "Societal Health & Safety"@en .

risk-owl:SocietalRiskConcept a rdfs:Class,
        owl:Class,
        dpv-owl:RiskConcept,
        risk-owl:PotentialConsequence,
        risk-owl:PotentialImpact,
        risk-owl:PotentialRisk,
        risk-owl:PotentialRiskSource ;
    dct:created "2024-10-21"^^xsd:date ;
    rdfs:isDefinedBy risk-owl: ;
    rdfs:subClassOf dpv-owl:RiskConcept ;
    sw:term_status "accepted"@en ;
    skos:definition "Risk concepts, including any potential risk sources, consequences, or impacts, that are societal in nature or relate to a social setting or process"@en ;
    skos:prefLabel "Societal Risk Concept"@en ;
    skos:scopeNote "Societal in this context includes both individuals and groups in a social context, as well as wider implications for society - such as environmental impacts or economic consequences of inflation that can affect both human and non-human entities as part of the social structure"@en .

risk-owl:SourceControl a rdfs:Class,
        owl:Class,
        risk-owl:RiskControl ;
    dct:contributor _:Ne22a67b17c7e4a779c30d2864b6a0cee ;
    dct:created "2024-05-19"^^xsd:date ;
    dct:modified "2025-01-06"^^xsd:date ;
    rdfs:isDefinedBy risk-owl: ;
    rdfs:subClassOf risk-owl:RiskControl ;
    sw:term_status "modified"@en ;
    skos:definition "Risk control for managing risk sources"@en ;
    skos:prefLabel "Source Control"@en .

risk-owl:Spoofing a rdfs:Class,
        owl:Class,
        dpv-owl:RiskConcept,
        risk-owl:ConfidentialityConcept,
        risk-owl:IntegrityConcept,
        risk-owl:PotentialConsequence,
        risk-owl:PotentialRisk,
        risk-owl:PotentialRiskSource ;
    dct:contributor _:Ne22a67b17c7e4a779c30d2864b6a0cee ;
    dct:created "2022-08-17"^^xsd:date ;
    dct:modified "2024-08-16"^^xsd:date ;
    dct:source [ a schema:WebPage ;
            schema:name "ISO/IEC 27005:2018" ;
            schema:url "https://www.iso.org/standard/75281.html" ] ;
    rdfs:isDefinedBy risk-owl: ;
    rdfs:subClassOf risk-owl:MaliciousActivity ;
    sw:term_status "accepted"@en ;
    skos:definition "Concept representing Spoofing"@en ;
    skos:prefLabel "Spoofing"@en .

risk-owl:StaffIncompetence a rdfs:Class,
        owl:Class,
        dpv-owl:RiskConcept,
        risk-owl:PotentialConsequence,
        risk-owl:PotentialRisk,
        risk-owl:PotentialRiskSource ;
    dct:contributor _:N9c63c24625fe482386a350b4ea27b4f8,
        _:Ne22a67b17c7e4a779c30d2864b6a0cee ;
    dct:created "2024-12-01"^^xsd:date ;
    rdfs:isDefinedBy risk-owl: ;
    rdfs:subClassOf risk-owl:OrganisationalManagementRisk ;
    sw:term_status "accepted"@en ;
    skos:definition "Concept representing incompetence of staff"@en ;
    skos:prefLabel "Staff Incompetence"@en .

risk-owl:StatisticalBias a rdfs:Class,
        owl:Class,
        dpv-owl:RiskConcept,
        risk-owl:PotentialConsequence,
        risk-owl:PotentialRisk,
        risk-owl:PotentialRiskSource ;
    dct:contributor _:N2e9307242cb14d528effb994db501842,
        _:N9c63c24625fe482386a350b4ea27b4f8,
        _:Ne22a67b17c7e4a779c30d2864b6a0cee ;
    dct:created "2024-09-13"^^xsd:date ;
    dct:source "ISO 20501:2019"@en ;
    rdfs:isDefinedBy risk-owl: ;
    rdfs:subClassOf risk-owl:DataBias ;
    sw:term_status "accepted"@en ;
    skos:definition "Bias that occurs as the type of consistent numerical offset in an estimate relative to the true underlying value, inherent to most estimates"@en ;
    skos:prefLabel "Statistical Bias"@en .

risk-owl:SubstitutionControl a rdfs:Class,
        owl:Class,
        risk-owl:RiskControl ;
    dct:contributor _:N9c63c24625fe482386a350b4ea27b4f8,
        _:Ne22a67b17c7e4a779c30d2864b6a0cee ;
    dct:created "2025-01-06"^^xsd:date ;
    rdfs:isDefinedBy risk-owl: ;
    rdfs:subClassOf risk-owl:AvoidanceControl ;
    sw:term_status "accepted"@en ;
    skos:definition "Control that substitutes an event with another such that the initial event no longer takes place while the substituted event takes place in place of it"@en ;
    skos:prefLabel "Substitution Control"@en ;
    skos:scopeNote "Substitution implies that the replacement event is less risky or is more safe than the replaced event, which is distinct from elimination where no event occurs and thus there is an elimination of risk entirely"@en .

risk-owl:SystemFailure a rdfs:Class,
        owl:Class,
        dpv-owl:RiskConcept,
        risk-owl:AvailabilityConcept,
        risk-owl:PotentialConsequence,
        risk-owl:PotentialRisk,
        risk-owl:PotentialRiskSource ;
    dct:contributor _:Ne22a67b17c7e4a779c30d2864b6a0cee ;
    dct:created "2022-08-17"^^xsd:date ;
    dct:modified "2024-08-16"^^xsd:date ;
    dct:source [ a schema:WebPage ;
            schema:name "ENISA Threat Landscape for Ransomware Attacks 2022" ;
            schema:url "https://www.enisa.europa.eu/publications/enisa-threat-landscape-for-ransomware-attacks" ] ;
    rdfs:isDefinedBy risk-owl: ;
    rdfs:subClassOf risk-owl:OperationalSecurityRisk ;
    sw:term_status "accepted"@en ;
    skos:definition "Concept representing System Failure"@en ;
    skos:prefLabel "System Failure"@en ;
    skos:scopeNote "Here system refers to both hardware and software systems"@en .

risk-owl:SystemIntrusion a rdfs:Class,
        owl:Class,
        dpv-owl:RiskConcept,
        risk-owl:AvailabilityConcept,
        risk-owl:ConfidentialityConcept,
        risk-owl:IntegrityConcept,
        risk-owl:PotentialRisk,
        risk-owl:PotentialRiskSource ;
    dct:contributor _:Ne22a67b17c7e4a779c30d2864b6a0cee ;
    dct:created "2022-08-17"^^xsd:date ;
    dct:modified "2024-08-16"^^xsd:date ;
    dct:source [ a schema:WebPage ;
            schema:name "ENISA Reference Incident Classification Taxonomy 2018" ;
            schema:url "https://www.enisa.europa.eu/publications/reference-incident-classification-taxonomy/" ] ;
    rdfs:isDefinedBy risk-owl: ;
    rdfs:subClassOf risk-owl:SecurityAttack ;
    sw:term_status "accepted"@en ;
    skos:definition "Concept representing System Intrusion"@en ;
    skos:prefLabel "System Intrusion"@en .

risk-owl:SystemMalfunction a rdfs:Class,
        owl:Class,
        dpv-owl:RiskConcept,
        risk-owl:AvailabilityConcept,
        risk-owl:PotentialConsequence,
        risk-owl:PotentialRisk,
        risk-owl:PotentialRiskSource ;
    dct:contributor _:Ne22a67b17c7e4a779c30d2864b6a0cee ;
    dct:created "2022-08-17"^^xsd:date ;
    dct:modified "2024-08-16"^^xsd:date ;
    dct:source [ a schema:WebPage ;
            schema:name "ISO/IEC 27005:2018" ;
            schema:url "https://www.iso.org/standard/75281.html" ] ;
    rdfs:isDefinedBy risk-owl: ;
    rdfs:subClassOf risk-owl:OperationalSecurityRisk ;
    sw:term_status "accepted"@en ;
    skos:definition "Concept representing System Malfunction"@en ;
    skos:prefLabel "System Malfunction"@en ;
    skos:scopeNote "Here system refers to both hardware and software systems"@en .

risk-owl:TaskExecutionIncorrect a rdfs:Class,
        owl:Class,
        dpv-owl:RiskConcept,
        risk-owl:AvailabilityConcept,
        risk-owl:IntegrityConcept,
        risk-owl:PotentialConsequence,
        risk-owl:PotentialRisk,
        risk-owl:PotentialRiskSource ;
    dct:contributor _:Ne22a67b17c7e4a779c30d2864b6a0cee ;
    dct:created "2024-12-01"^^xsd:date ;
    rdfs:isDefinedBy risk-owl: ;
    rdfs:subClassOf risk-owl:TaskExecutionRisk ;
    sw:term_status "accepted"@en ;
    skos:definition "Concept representing incorrect execution of task(s)"@en ;
    skos:prefLabel "Task Execution Incorrect"@en .

risk-owl:TaskExecutionRisk a rdfs:Class,
        owl:Class,
        dpv-owl:RiskConcept,
        risk-owl:IntegrityConcept,
        risk-owl:PotentialConsequence,
        risk-owl:PotentialRisk,
        risk-owl:PotentialRiskSource ;
    dct:contributor _:Ne22a67b17c7e4a779c30d2864b6a0cee ;
    dct:created "2024-12-01"^^xsd:date ;
    rdfs:isDefinedBy risk-owl: ;
    rdfs:subClassOf risk-owl:OperationalSecurityRisk ;
    sw:term_status "accepted"@en ;
    skos:definition "Concept representing risks and issues associated with execution of tasks, operations, activities, and other similar processes"@en ;
    skos:prefLabel "Task Execution Risk"@en .

risk-owl:TaskOmmitted a rdfs:Class,
        owl:Class,
        dpv-owl:RiskConcept,
        risk-owl:AvailabilityConcept,
        risk-owl:IntegrityConcept,
        risk-owl:PotentialConsequence,
        risk-owl:PotentialRisk,
        risk-owl:PotentialRiskSource ;
    dct:contributor _:Ne22a67b17c7e4a779c30d2864b6a0cee ;
    dct:created "2024-12-01"^^xsd:date ;
    rdfs:isDefinedBy risk-owl: ;
    rdfs:subClassOf risk-owl:TaskExecutionRisk ;
    sw:term_status "accepted"@en ;
    skos:definition "Concept representing omission of task(s)"@en ;
    skos:prefLabel "Task Ommitted"@en .

risk-owl:TaskTimingIncorrect a rdfs:Class,
        owl:Class,
        dpv-owl:RiskConcept,
        risk-owl:AvailabilityConcept,
        risk-owl:IntegrityConcept,
        risk-owl:PotentialConsequence,
        risk-owl:PotentialRisk,
        risk-owl:PotentialRiskSource ;
    dct:contributor _:Ne22a67b17c7e4a779c30d2864b6a0cee ;
    dct:created "2024-12-01"^^xsd:date ;
    rdfs:isDefinedBy risk-owl: ;
    rdfs:subClassOf risk-owl:TaskExecutionRisk ;
    sw:term_status "accepted"@en ;
    skos:definition "Concept representing incorrect timing for task(s) i.e. the task execution does not occur at the correct time"@en ;
    skos:prefLabel "Task Timing Incorrect"@en .

risk-owl:TechnicalRiskConcept a rdfs:Class,
        owl:Class,
        dpv-owl:RiskConcept,
        risk-owl:PotentialConsequence,
        risk-owl:PotentialImpact,
        risk-owl:PotentialRisk,
        risk-owl:PotentialRiskSource ;
    dct:created "2025-01-06"^^xsd:date ;
    rdfs:isDefinedBy risk-owl: ;
    rdfs:subClassOf dpv-owl:RiskConcept ;
    sw:term_status "accepted"@en ;
    skos:definition "Risk concepts, including any potential risk sources, consequences, or impacts, that are technical in nature or relate to a technical or technological process"@en ;
    skos:prefLabel "Technical Risk Concept"@en .

risk-owl:TechnologyOverreliance a rdfs:Class,
        owl:Class,
        dpv-owl:RiskConcept,
        risk-owl:PotentialConsequence,
        risk-owl:PotentialRisk,
        risk-owl:PotentialRiskSource ;
    dct:contributor _:N9c63c24625fe482386a350b4ea27b4f8,
        _:Ne22a67b17c7e4a779c30d2864b6a0cee ;
    dct:created "2024-12-01"^^xsd:date ;
    rdfs:isDefinedBy risk-owl: ;
    rdfs:subClassOf risk-owl:OrganisationalManagementRisk ;
    sw:term_status "accepted"@en ;
    skos:definition "Concept representing the case where an entity, including individuals, have an overreliance on the use of technology"@en ;
    skos:prefLabel "Technology Overreliance"@en .

risk-owl:Terrorism a rdfs:Class,
        owl:Class,
        dpv-owl:RiskConcept,
        risk-owl:PotentialConsequence,
        risk-owl:PotentialImpact,
        risk-owl:PotentialRisk ;
    dct:contributor _:Ne22a67b17c7e4a779c30d2864b6a0cee ;
    dct:created "2022-08-17"^^xsd:date ;
    dct:modified "2024-08-16"^^xsd:date ;
    dct:source [ a schema:WebPage ;
            schema:name "ISO/IEC 27005:2018" ;
            schema:url "https://www.iso.org/standard/75281.html" ] ;
    rdfs:isDefinedBy risk-owl: ;
    rdfs:subClassOf risk-owl:GroupRisk ;
    sw:term_status "accepted"@en ;
    skos:definition "Concept representing Terrorism"@en ;
    skos:prefLabel "Terrorism"@en .

risk-owl:Threat a rdfs:Class,
        owl:Class ;
    dct:created "2024-02-14"^^xsd:date ;
    rdfs:isDefinedBy risk-owl: ;
    rdfs:subClassOf risk-owl:RiskIdentification ;
    sw:term_status "accepted"@en ;
    skos:definition "Risk source event which causes Risk"@en ;
    skos:prefLabel "Threat"@en .

risk-owl:ThreatSource a rdfs:Class,
        owl:Class ;
    dct:created "2024-02-14"^^xsd:date ;
    rdfs:isDefinedBy risk-owl: ;
    rdfs:subClassOf risk-owl:RiskIdentification ;
    sw:term_status "accepted"@en ;
    skos:definition "Source of threat event, including both agent and non-agent sources"@en ;
    skos:prefLabel "Threat Source"@en .

risk-owl:TransferControl a rdfs:Class,
        owl:Class,
        risk-owl:RiskControl ;
    dct:contributor _:Ne22a67b17c7e4a779c30d2864b6a0cee ;
    dct:created "2025-01-06"^^xsd:date ;
    rdfs:isDefinedBy risk-owl: ;
    rdfs:subClassOf risk-owl:RiskControl ;
    sw:term_status "accepted"@en ;
    skos:definition "Control that aims to transfer the event (or risk) to another context or entity"@en ;
    skos:prefLabel "Transfer Control"@en ;
    skos:scopeNote "Transfer implies moving (physically or logically) the event to another context or entity. While Risk Management methods indicate risk transfer as occuring between entities, this concept is defined more broadly by including 'context or entity' so as to enable modelling cases where the transfer takes place between processes - which may be managed by the same or different entity. Additionally, typical use of 'Transfer' implies a formal mechanism such as an agreement, which is absent from this concept. If only partial responsibility is tranferred, such as for a specific measure, then this can be considered as an instance of sharing the risk - for which risk:ShareControl is provided"@en .

risk-owl:TransparencyControl a rdfs:Class,
        owl:Class,
        risk-owl:RiskControl ;
    dct:contributor _:N9c63c24625fe482386a350b4ea27b4f8,
        _:Ne22a67b17c7e4a779c30d2864b6a0cee ;
    dct:created "2025-01-06"^^xsd:date ;
    rdfs:isDefinedBy risk-owl: ;
    rdfs:subClassOf risk-owl:MonitorControl ;
    sw:term_status "accepted"@en ;
    skos:definition "Control that provides information about an event"@en ;
    skos:prefLabel "Transparency Control"@en ;
    skos:scopeNote "Transparency refers to the availability of information, whether for the same or different entity in relation to who establishes and operates the control, and where transparency implies having the means to obtain and use information about an event"@en .

risk-owl:Transphobia a rdfs:Class,
        owl:Class,
        dpv-owl:RiskConcept,
        risk-owl:PotentialConsequence,
        risk-owl:PotentialImpact,
        risk-owl:PotentialRisk ;
    dct:created "2024-09-30"^^xsd:date ;
    rdfs:isDefinedBy risk-owl: ;
    rdfs:subClassOf risk-owl:Sexism ;
    sw:term_status "accepted"@en ;
    skos:definition "Hostility or prejudice against transgender people or those perceived as not conforming to traditional gender norms"@en ;
    skos:prefLabel "Transphobia"@en .

risk-owl:UnauthorisedAccesstoPremises a rdfs:Class,
        owl:Class,
        dpv-owl:RiskConcept,
        risk-owl:AvailabilityConcept,
        risk-owl:ConfidentialityConcept,
        risk-owl:IntegrityConcept,
        risk-owl:PotentialConsequence,
        risk-owl:PotentialRisk,
        risk-owl:PotentialRiskSource ;
    dct:contributor _:Ne22a67b17c7e4a779c30d2864b6a0cee ;
    dct:created "2022-08-17"^^xsd:date ;
    dct:modified "2024-08-16"^^xsd:date ;
    dct:source [ a schema:WebPage ;
            schema:name "ISO/IEC 27005:2018" ;
            schema:url "https://www.iso.org/standard/75281.html" ] ;
    rdfs:isDefinedBy risk-owl: ;
    rdfs:subClassOf risk-owl:UnauthorisedActivity ;
    sw:term_status "accepted"@en ;
    skos:definition "Concept representing Unauthorised Access to Premises"@en ;
    skos:prefLabel "Unauthorised Access to Premises"@en .

risk-owl:UnauthorisedActivity a rdfs:Class,
        owl:Class,
        dpv-owl:RiskConcept,
        risk-owl:AvailabilityConcept,
        risk-owl:ConfidentialityConcept,
        risk-owl:IntegrityConcept,
        risk-owl:PotentialConsequence,
        risk-owl:PotentialRisk,
        risk-owl:PotentialRiskSource ;
    dct:created "2024-12-17"^^xsd:date ;
    rdfs:isDefinedBy risk-owl: ;
    rdfs:subClassOf risk-owl:ExternalSecurityThreat ;
    sw:term_status "accepted"@en ;
    skos:definition "Concept representing Unauthorised Activity"@en ;
    skos:prefLabel "Unauthorised Activity"@en .

risk-owl:UnauthorisedCodeAccess a rdfs:Class,
        owl:Class,
        dpv-owl:RiskConcept,
        risk-owl:ConfidentialityConcept,
        risk-owl:IntegrityConcept,
        risk-owl:PotentialConsequence,
        risk-owl:PotentialRisk,
        risk-owl:PotentialRiskSource ;
    dct:contributor _:Ne22a67b17c7e4a779c30d2864b6a0cee ;
    dct:created "2022-08-17"^^xsd:date ;
    dct:modified "2024-08-16"^^xsd:date ;
    dct:source [ a schema:WebPage ;
            schema:name "ENISA Methodology for Sectoral Cybersecurity Assessments" ;
            schema:url "https://www.enisa.europa.eu/publications/methodology-for-a-sectoral-cybersecurity-assessment" ] ;
    rdfs:isDefinedBy risk-owl: ;
    rdfs:subClassOf risk-owl:UnauthorisedActivity ;
    sw:term_status "accepted"@en ;
    skos:definition "Concept representing Unauthorised Code Access"@en ;
    skos:prefLabel "Unauthorised Code Access"@en .

risk-owl:UnauthorisedCodeDisclosure a rdfs:Class,
        owl:Class,
        dpv-owl:RiskConcept,
        risk-owl:ConfidentialityConcept,
        risk-owl:PotentialConsequence,
        risk-owl:PotentialRisk,
        risk-owl:PotentialRiskSource ;
    dct:contributor _:Ne22a67b17c7e4a779c30d2864b6a0cee ;
    dct:created "2022-08-17"^^xsd:date ;
    dct:modified "2024-08-16"^^xsd:date ;
    dct:source [ a schema:WebPage ;
            schema:name "ENISA Methodology for Sectoral Cybersecurity Assessments" ;
            schema:url "https://www.enisa.europa.eu/publications/methodology-for-a-sectoral-cybersecurity-assessment" ] ;
    rdfs:isDefinedBy risk-owl: ;
    rdfs:subClassOf risk-owl:UnauthorisedActivity ;
    sw:term_status "accepted"@en ;
    skos:definition "Concept representing Unauthorised Code Disclosure"@en ;
    skos:prefLabel "Unauthorised Code Disclosure"@en .

risk-owl:UnauthorisedCodeModification a rdfs:Class,
        owl:Class,
        dpv-owl:RiskConcept,
        risk-owl:IntegrityConcept,
        risk-owl:PotentialConsequence,
        risk-owl:PotentialRisk,
        risk-owl:PotentialRiskSource ;
    dct:contributor _:Ne22a67b17c7e4a779c30d2864b6a0cee ;
    dct:created "2022-08-17"^^xsd:date ;
    dct:modified "2024-08-16"^^xsd:date ;
    dct:source [ a schema:WebPage ;
            schema:name "ENISA Methodology for Sectoral Cybersecurity Assessments" ;
            schema:url "https://www.enisa.europa.eu/publications/methodology-for-a-sectoral-cybersecurity-assessment" ] ;
    rdfs:isDefinedBy risk-owl: ;
    rdfs:subClassOf risk-owl:UnauthorisedActivity ;
    sw:term_status "accepted"@en ;
    skos:definition "Concept representing Unauthorised Code Modification"@en ;
    skos:prefLabel "Unauthorised Code Modification"@en .

risk-owl:UnauthorisedDataAccess a rdfs:Class,
        owl:Class,
        dpv-owl:RiskConcept,
        risk-owl:ConfidentialityConcept,
        risk-owl:PotentialConsequence,
        risk-owl:PotentialRisk,
        risk-owl:PotentialRiskSource ;
    dct:contributor _:Ne22a67b17c7e4a779c30d2864b6a0cee ;
    dct:created "2022-08-17"^^xsd:date ;
    dct:modified "2024-08-16"^^xsd:date ;
    dct:source [ a schema:WebPage ;
            schema:name "ENISA Reference Incident Classification Taxonomy 2018" ;
            schema:url "https://www.enisa.europa.eu/publications/reference-incident-classification-taxonomy/" ] ;
    rdfs:isDefinedBy risk-owl: ;
    rdfs:subClassOf risk-owl:UnauthorisedActivity ;
    sw:term_status "accepted"@en ;
    skos:definition "Concept representing Unauthorised Data Access"@en ;
    skos:prefLabel "Unauthorised Data Access"@en .

risk-owl:UnauthorisedDataDisclosure a rdfs:Class,
        owl:Class,
        dpv-owl:RiskConcept,
        risk-owl:ConfidentialityConcept,
        risk-owl:PotentialConsequence,
        risk-owl:PotentialRisk,
        risk-owl:PotentialRiskSource ;
    dct:contributor _:Ne22a67b17c7e4a779c30d2864b6a0cee ;
    dct:created "2022-08-17"^^xsd:date ;
    dct:modified "2024-08-16"^^xsd:date ;
    dct:source [ a schema:WebPage ;
            schema:name "ISO/IEC 27005:2018" ;
            schema:url "https://www.iso.org/standard/75281.html" ] ;
    rdfs:isDefinedBy risk-owl: ;
    rdfs:subClassOf risk-owl:UnauthorisedActivity ;
    sw:term_status "accepted"@en ;
    skos:definition "Concept representing Unauthorised Data Disclosure"@en ;
    skos:prefLabel "Unauthorised Data Disclosure"@en .

risk-owl:UnauthorisedDataModification a rdfs:Class,
        owl:Class,
        dpv-owl:RiskConcept,
        risk-owl:IntegrityConcept,
        risk-owl:PotentialConsequence,
        risk-owl:PotentialRisk,
        risk-owl:PotentialRiskSource ;
    dct:contributor _:Ne22a67b17c7e4a779c30d2864b6a0cee ;
    dct:created "2022-08-17"^^xsd:date ;
    dct:modified "2024-08-16"^^xsd:date ;
    dct:source [ a schema:WebPage ;
            schema:name "ENISA Reference Incident Classification Taxonomy 2018" ;
            schema:url "https://www.enisa.europa.eu/publications/reference-incident-classification-taxonomy/" ] ;
    rdfs:isDefinedBy risk-owl: ;
    rdfs:subClassOf risk-owl:UnauthorisedActivity ;
    sw:term_status "accepted"@en ;
    skos:definition "Concept representing Unauthorised Data Modification"@en ;
    skos:prefLabel "Unauthorised Data Modification"@en .

risk-owl:UnauthorisedInformationDisclosure a rdfs:Class,
        owl:Class,
        dpv-owl:RiskConcept,
        risk-owl:ConfidentialityConcept,
        risk-owl:PotentialConsequence,
        risk-owl:PotentialRisk,
        risk-owl:PotentialRiskSource ;
    dct:contributor _:Ne22a67b17c7e4a779c30d2864b6a0cee ;
    dct:created "2022-08-17"^^xsd:date ;
    dct:modified "2024-08-16"^^xsd:date ;
    dct:source [ a schema:WebPage ;
            schema:name "ENISA Reference Incident Classification Taxonomy 2018" ;
            schema:url "https://www.enisa.europa.eu/publications/reference-incident-classification-taxonomy/" ] ;
    rdfs:isDefinedBy risk-owl: ;
    rdfs:subClassOf risk-owl:UnauthorisedActivity ;
    sw:term_status "accepted"@en ;
    skos:definition "Concept representing Unauthorised Information Disclosure"@en ;
    skos:prefLabel "Unauthorised Information Disclosure"@en .

risk-owl:UnauthorisedReidentification a rdfs:Class,
        owl:Class,
        dpv-owl:RiskConcept,
        risk-owl:ConfidentialityConcept,
        risk-owl:PotentialConsequence,
        risk-owl:PotentialRisk,
        risk-owl:PotentialRiskSource ;
    dct:contributor _:N7d9b5ee7f31f4f2ba5951e30b49ec7c0 ;
    dct:created "2022-08-19"^^xsd:date ;
    dct:modified "2024-08-16"^^xsd:date ;
    rdfs:isDefinedBy risk-owl: ;
    rdfs:subClassOf risk-owl:UnauthorisedActivity ;
    sw:term_status "accepted"@en ;
    skos:definition "Concept representing Unauthorised Re-Identification"@en ;
    skos:prefLabel "Unauthorised Re-Identification"@en .

risk-owl:UnauthorisedResourceUse a rdfs:Class,
        owl:Class,
        dpv-owl:RiskConcept,
        risk-owl:AvailabilityConcept,
        risk-owl:PotentialConsequence,
        risk-owl:PotentialRisk,
        risk-owl:PotentialRiskSource ;
    dct:contributor _:Ne22a67b17c7e4a779c30d2864b6a0cee ;
    dct:created "2022-08-17"^^xsd:date ;
    dct:modified "2024-08-16"^^xsd:date ;
    dct:source [ a schema:WebPage ;
            schema:name "ISO/IEC 27005:2018" ;
            schema:url "https://www.iso.org/standard/75281.html" ] ;
    rdfs:isDefinedBy risk-owl: ;
    rdfs:subClassOf risk-owl:UnauthorisedActivity ;
    sw:term_status "accepted"@en ;
    skos:definition "Concept representing Unauthorised Resource Use"@en ;
    skos:prefLabel "Unauthorised Resource Use"@en .

risk-owl:UnauthorisedSystemAccess a rdfs:Class,
        owl:Class,
        dpv-owl:RiskConcept,
        risk-owl:ConfidentialityConcept,
        risk-owl:IntegrityConcept,
        risk-owl:PotentialConsequence,
        risk-owl:PotentialRisk,
        risk-owl:PotentialRiskSource ;
    dct:contributor _:Ne22a67b17c7e4a779c30d2864b6a0cee ;
    dct:created "2022-08-17"^^xsd:date ;
    dct:modified "2024-08-16"^^xsd:date ;
    dct:source [ a schema:WebPage ;
            schema:name "ISO/IEC 27005:2018" ;
            schema:url "https://www.iso.org/standard/75281.html" ] ;
    rdfs:isDefinedBy risk-owl: ;
    rdfs:subClassOf risk-owl:UnauthorisedActivity ;
    sw:term_status "accepted"@en ;
    skos:definition "Concept representing Unauthorised System Access"@en ;
    skos:prefLabel "Unauthorised System Access"@en .

risk-owl:UnauthorisedSystemModification a rdfs:Class,
        owl:Class,
        dpv-owl:RiskConcept,
        risk-owl:IntegrityConcept,
        risk-owl:PotentialConsequence,
        risk-owl:PotentialRisk,
        risk-owl:PotentialRiskSource ;
    dct:contributor _:Ne22a67b17c7e4a779c30d2864b6a0cee ;
    dct:created "2022-08-17"^^xsd:date ;
    dct:modified "2024-08-16"^^xsd:date ;
    dct:source [ a schema:WebPage ;
            schema:name "ENISA Methodology for Sectoral Cybersecurity Assessments" ;
            schema:url "https://www.enisa.europa.eu/publications/methodology-for-a-sectoral-cybersecurity-assessment" ] ;
    rdfs:isDefinedBy risk-owl: ;
    rdfs:subClassOf risk-owl:UnauthorisedActivity ;
    sw:term_status "accepted"@en ;
    skos:definition "Concept representing Unauthorised System Modification"@en ;
    skos:prefLabel "Unauthorised System Modification"@en .

risk-owl:UnwantedCodeDeletion a rdfs:Class,
        owl:Class,
        dpv-owl:RiskConcept,
        risk-owl:AvailabilityConcept,
        risk-owl:IntegrityConcept,
        risk-owl:PotentialConsequence,
        risk-owl:PotentialRisk,
        risk-owl:PotentialRiskSource ;
    dct:contributor _:Ne22a67b17c7e4a779c30d2864b6a0cee ;
    dct:created "2022-08-17"^^xsd:date ;
    dct:modified "2024-08-16"^^xsd:date ;
    dct:source [ a schema:WebPage ;
            schema:name "ENISA Methodology for Sectoral Cybersecurity Assessments" ;
            schema:url "https://www.enisa.europa.eu/publications/methodology-for-a-sectoral-cybersecurity-assessment" ] ;
    rdfs:isDefinedBy risk-owl: ;
    rdfs:subClassOf risk-owl:UnauthorisedActivity ;
    sw:term_status "accepted"@en ;
    skos:definition "Concept representing Unwanted Code Deletion"@en ;
    skos:prefLabel "Unwanted Code Deletion"@en .

risk-owl:UnwantedDataDeletion a rdfs:Class,
        owl:Class,
        dpv-owl:RiskConcept,
        risk-owl:AvailabilityConcept,
        risk-owl:IntegrityConcept,
        risk-owl:PotentialConsequence,
        risk-owl:PotentialRisk,
        risk-owl:PotentialRiskSource ;
    dct:contributor _:Ne22a67b17c7e4a779c30d2864b6a0cee ;
    dct:created "2022-08-17"^^xsd:date ;
    dct:modified "2024-08-16"^^xsd:date ;
    dct:source [ a schema:WebPage ;
            schema:name "ISO/IEC 27005:2018" ;
            schema:url "https://www.iso.org/standard/75281.html" ] ;
    rdfs:isDefinedBy risk-owl: ;
    rdfs:subClassOf risk-owl:UnauthorisedActivity ;
    sw:term_status "accepted"@en ;
    skos:definition "Concept representing Unwanted Data Deletion"@en ;
    skos:prefLabel "Unwanted Data Deletion"@en .

risk-owl:UnwantedDisclosureData a rdfs:Class,
        owl:Class,
        dpv-owl:RiskConcept,
        risk-owl:ConfidentialityConcept,
        risk-owl:PotentialConsequence,
        risk-owl:PotentialRisk,
        risk-owl:PotentialRiskSource ;
    dct:contributor _:Ne22a67b17c7e4a779c30d2864b6a0cee ;
    dct:created "2022-08-17"^^xsd:date ;
    dct:modified "2024-08-16"^^xsd:date ;
    dct:source [ a schema:WebPage ;
            schema:name "ISO/IEC 27005:2018" ;
            schema:url "https://www.iso.org/standard/75281.html" ] ;
    rdfs:isDefinedBy risk-owl: ;
    rdfs:subClassOf risk-owl:UnauthorisedActivity ;
    sw:term_status "accepted"@en ;
    skos:definition "Concept representing Unwanted Disclosure of Data"@en ;
    skos:prefLabel "Unwanted Disclosure of Data"@en .

risk-owl:UserRisks a rdfs:Class,
        owl:Class,
        dpv-owl:RiskConcept,
        risk-owl:PotentialConsequence,
        risk-owl:PotentialRisk,
        risk-owl:PotentialRiskSource ;
    dct:created "2024-12-17"^^xsd:date ;
    rdfs:isDefinedBy risk-owl: ;
    rdfs:subClassOf risk-owl:OrganisationalRiskConcept ;
    sw:term_status "accepted"@en ;
    skos:definition "Concepts associated with risks that arise due to User or Human use"@en ;
    skos:prefLabel "User Risks"@en .

risk-owl:VeryHighLikelihood a rdfs:Class,
        owl:Class,
        dpv-owl:Likelihood ;
    dct:contributor _:Ne22a67b17c7e4a779c30d2864b6a0cee ;
    dct:created "2022-08-18"^^xsd:date ;
    rdf:value "0.9,xsd:decimal" ;
    rdfs:isDefinedBy risk-owl: ;
    rdfs:subClassOf risk-owl:5LikelihoodLevels,
        risk-owl:7LikelihoodLevels ;
    sw:term_status "accepted"@en ;
    skos:definition "Level where Likelihood is Very High"@en ;
    skos:prefLabel "Very High Likelihood"@en ;
    skos:scopeNote "The suggested quantitative value for this concept is 0.9 on a scale of 0 to 1"@en .

risk-owl:VeryHighRisk a rdfs:Class,
        owl:Class,
        dpv-owl:RiskLevel ;
    dct:contributor _:Ne22a67b17c7e4a779c30d2864b6a0cee ;
    dct:created "2022-08-18"^^xsd:date ;
    rdf:value "0.9,xsd:decimal" ;
    rdfs:isDefinedBy risk-owl: ;
    rdfs:subClassOf risk-owl:5RiskLevels,
        risk-owl:7RiskLevels ;
    sw:term_status "accepted"@en ;
    skos:definition "Level where Risk is Very High"@en ;
    skos:prefLabel "Very High Risk"@en ;
    skos:scopeNote "The suggested quantitative value for this concept is 0.9 on a scale of 0 to 1"@en .

risk-owl:VeryHighSeverity a rdfs:Class,
        owl:Class,
        dpv-owl:Severity ;
    dct:contributor _:Ne22a67b17c7e4a779c30d2864b6a0cee ;
    dct:created "2022-08-18"^^xsd:date ;
    rdf:value "0.9,xsd:decimal" ;
    rdfs:isDefinedBy risk-owl: ;
    rdfs:subClassOf risk-owl:5SeverityLevels,
        risk-owl:7SeverityLevels ;
    sw:term_status "accepted"@en ;
    skos:definition "Level where Severity is Very High"@en ;
    skos:prefLabel "Very High Severity"@en ;
    skos:scopeNote "The suggested quantitative value for this concept is 0.9 on a scale of 0 to 1"@en .

risk-owl:VeryLowLikelihood a rdfs:Class,
        owl:Class,
        dpv-owl:Likelihood ;
    dct:contributor _:Ne22a67b17c7e4a779c30d2864b6a0cee ;
    dct:created "2022-08-18"^^xsd:date ;
    rdf:value "0.1,xsd:decimal" ;
    rdfs:isDefinedBy risk-owl: ;
    rdfs:subClassOf risk-owl:5LikelihoodLevels,
        risk-owl:7LikelihoodLevels ;
    sw:term_status "accepted"@en ;
    skos:definition "Level where Likelihood is Very Low"@en ;
    skos:prefLabel "Very Low Likelihood"@en ;
    skos:scopeNote "The suggested quantitative value for this concept is 0.1 on a scale of 0 to 1"@en .

risk-owl:VeryLowRisk a rdfs:Class,
        owl:Class,
        dpv-owl:RiskLevel ;
    dct:contributor _:Ne22a67b17c7e4a779c30d2864b6a0cee ;
    dct:created "2022-08-18"^^xsd:date ;
    rdf:value "0.1,xsd:decimal" ;
    rdfs:isDefinedBy risk-owl: ;
    rdfs:subClassOf risk-owl:5RiskLevels,
        risk-owl:7RiskLevels ;
    sw:term_status "accepted"@en ;
    skos:definition "Level where Risk is Very Low"@en ;
    skos:prefLabel "Very Low Risk"@en ;
    skos:scopeNote "The suggested quantitative value for this concept is 0.1 on a scale of 0 to 1"@en .

risk-owl:VeryLowSeverity a rdfs:Class,
        owl:Class,
        dpv-owl:Severity ;
    dct:contributor _:Ne22a67b17c7e4a779c30d2864b6a0cee ;
    dct:created "2022-08-18"^^xsd:date ;
    rdf:value "0.1,xsd:decimal" ;
    rdfs:isDefinedBy risk-owl: ;
    rdfs:subClassOf risk-owl:5SeverityLevels,
        risk-owl:7SeverityLevels ;
    sw:term_status "accepted"@en ;
    skos:definition "Level where Severity is Very Low"@en ;
    skos:prefLabel "Very Low Severity"@en ;
    skos:scopeNote "The suggested quantitative value for this concept is 0.1 on a scale of 0 to 1"@en .

risk-owl:ViolatingCodeOfConduct a rdfs:Class,
        owl:Class,
        dpv-owl:RiskConcept,
        risk-owl:PotentialConsequence,
        risk-owl:PotentialRisk ;
    dct:contributor _:Ne22a67b17c7e4a779c30d2864b6a0cee ;
    dct:created "2022-08-17"^^xsd:date ;
    dct:modified "2024-08-16"^^xsd:date ;
    dct:source [ a schema:WebPage ;
            schema:name "ISO/IEC 27005:2018" ;
            schema:url "https://www.iso.org/standard/75281.html" ] ;
    rdfs:isDefinedBy risk-owl: ;
    rdfs:subClassOf risk-owl:PolicyRisk ;
    sw:term_status "modified"@en ;
    skos:definition "Concept representing Violation of Code of Conduct"@en ;
    skos:prefLabel "Violating Code of Conduct"@en ;
    skos:scopeNote "This concept was called \"ViolationCodeConduct\" in DPV 2.0"@en .

risk-owl:ViolatingContractualObligation a rdfs:Class,
        owl:Class,
        dpv-owl:RiskConcept,
        risk-owl:PotentialConsequence,
        risk-owl:PotentialRisk ;
    dct:contributor _:Ne22a67b17c7e4a779c30d2864b6a0cee ;
    dct:created "2022-08-17"^^xsd:date ;
    dct:modified "2024-08-16"^^xsd:date ;
    dct:source [ a schema:WebPage ;
            schema:name "ISO/IEC 27005:2018" ;
            schema:url "https://www.iso.org/standard/75281.html" ] ;
    rdfs:isDefinedBy risk-owl: ;
    rdfs:subClassOf risk-owl:LegalComplianceRisk,
        risk-owl:ViolatingObligation ;
    sw:term_status "modified"@en ;
    skos:definition "Concept representing Violation of Contractual Obligations"@en ;
    skos:prefLabel "Violating Contractual Obligation"@en ;
    skos:scopeNote "This concept was called \"ViolationContractualObligations\" in DPV 2.0"@en .

risk-owl:ViolatingEthicsCode a rdfs:Class,
        owl:Class,
        dpv-owl:RiskConcept,
        risk-owl:PotentialConsequence,
        risk-owl:PotentialRisk ;
    dct:contributor _:Ne22a67b17c7e4a779c30d2864b6a0cee ;
    dct:created "2022-08-17"^^xsd:date ;
    dct:modified "2024-08-16"^^xsd:date ;
    dct:source [ a schema:WebPage ;
            schema:name "ISO/IEC 27005:2018" ;
            schema:url "https://www.iso.org/standard/75281.html" ] ;
    rdfs:isDefinedBy risk-owl: ;
    rdfs:subClassOf risk-owl:PolicyRisk ;
    sw:term_status "modified"@en ;
    skos:definition "Concept representing Violation of Ethics Code"@en ;
    skos:prefLabel "Violating Ethics Code"@en ;
    skos:scopeNote "This concept was called \"ViolationEthicalCode\" in DPV 2.0"@en .

risk-owl:ViolatingLegalObligation a rdfs:Class,
        owl:Class,
        dpv-owl:RiskConcept,
        risk-owl:PotentialConsequence,
        risk-owl:PotentialRisk ;
    dct:contributor _:Ne22a67b17c7e4a779c30d2864b6a0cee ;
    dct:created "2022-08-17"^^xsd:date ;
    dct:modified "2024-08-16"^^xsd:date ;
    dct:source [ a schema:WebPage ;
            schema:name "ISO/IEC 27005:2018" ;
            schema:url "https://www.iso.org/standard/75281.html" ] ;
    rdfs:isDefinedBy risk-owl: ;
    rdfs:subClassOf risk-owl:LegalComplianceRisk,
        risk-owl:ViolatingObligation ;
    sw:term_status "modified"@en ;
    skos:definition "Concept representing Violation of Legal Obligations"@en ;
    skos:prefLabel "Violating Legal Obligation"@en ;
    skos:scopeNote "This concept was called \"ViolationRegulatoryObligations\" in DPV 2.0"@en .

risk-owl:ViolatingObligation a rdfs:Class,
        owl:Class,
        dpv-owl:RiskConcept,
        risk-owl:PotentialConsequence,
        risk-owl:PotentialRisk ;
    dct:created "2024-10-21"^^xsd:date ;
    rdfs:isDefinedBy risk-owl: ;
    rdfs:subClassOf risk-owl:PolicyRisk ;
    sw:term_status "accepted"@en ;
    skos:definition "Something that acts as a or violates an obligation - e.g. in a law, code of conduct, policy, contract"@en ;
    skos:prefLabel "Violating Obligation"@en .

risk-owl:ViolatingPolicy a rdfs:Class,
        owl:Class,
        dpv-owl:RiskConcept,
        risk-owl:PotentialConsequence,
        risk-owl:PotentialRisk ;
    dct:created "2024-12-17"^^xsd:date ;
    rdfs:isDefinedBy risk-owl: ;
    rdfs:subClassOf risk-owl:PolicyRisk ;
    sw:term_status "accepted"@en ;
    skos:definition "Concept representing violation of policy which can be either internal or external policy"@en ;
    skos:prefLabel "Violating Policy"@en .

risk-owl:ViolatingProhibition a rdfs:Class,
        owl:Class,
        dpv-owl:RiskConcept,
        risk-owl:PotentialConsequence,
        risk-owl:PotentialRisk ;
    dct:created "2024-10-21"^^xsd:date ;
    rdfs:isDefinedBy risk-owl: ;
    rdfs:subClassOf risk-owl:PolicyRisk ;
    sw:term_status "accepted"@en ;
    skos:definition "Something that acts as a or violates a prohibition - e.g. in a law, code of conduct, policy, contract"@en ;
    skos:prefLabel "Violating Prohibition"@en .

risk-owl:ViolatingStatutoryObligations a rdfs:Class,
        owl:Class,
        dpv-owl:RiskConcept,
        risk-owl:PotentialConsequence,
        risk-owl:PotentialRisk ;
    dct:contributor _:Ne22a67b17c7e4a779c30d2864b6a0cee ;
    dct:created "2022-08-17"^^xsd:date ;
    dct:modified "2024-08-16"^^xsd:date ;
    dct:source [ a schema:WebPage ;
            schema:name "ISO/IEC 27005:2018" ;
            schema:url "https://www.iso.org/standard/75281.html" ] ;
    rdfs:isDefinedBy risk-owl: ;
    rdfs:subClassOf risk-owl:LegalComplianceRisk,
        risk-owl:ViolatingObligation ;
    sw:term_status "modified"@en ;
    skos:definition "Concept representing Violation of Statutory Obligations"@en ;
    skos:prefLabel "Violating Statutory Obligations"@en ;
    skos:scopeNote "This concept was called \"ViolationStatutoryObligations\" in DPV 2.0"@en .

risk-owl:ViolenceAgainstChildren a rdfs:Class,
        owl:Class,
        dpv-owl:RiskConcept,
        risk-owl:PotentialConsequence,
        risk-owl:PotentialImpact,
        risk-owl:PotentialRisk ;
    dct:contributor _:Ne22a67b17c7e4a779c30d2864b6a0cee ;
    dct:created "2022-08-17"^^xsd:date ;
    dct:modified "2024-08-16"^^xsd:date ;
    dct:source [ a schema:WebPage ;
            schema:name "ENISA Reference Incident Classification Taxonomy 2018" ;
            schema:url "https://www.enisa.europa.eu/publications/reference-incident-classification-taxonomy/" ] ;
    rdfs:isDefinedBy risk-owl: ;
    rdfs:subClassOf risk-owl:Harm ;
    sw:term_status "accepted"@en ;
    skos:definition "Concept representing Child Violence"@en ;
    skos:prefLabel "Violence against children"@en ;
    skos:scopeNote "This concept was called \"ChildViolence\" in DPV 2.0"@en .

risk-owl:Vulnerability a rdfs:Class,
        owl:Class ;
    dct:created "2024-02-14"^^xsd:date ;
    rdfs:isDefinedBy risk-owl: ;
    rdfs:subClassOf risk-owl:RiskIdentification ;
    sw:term_status "accepted"@en ;
    skos:definition "Intrinsic property of a system or asset that is utilised by the Threat Source in a Threat event to cause Risk"@en ;
    skos:prefLabel "Vulnerability"@en .

risk-owl:Wellbeing a rdfs:Class,
        owl:Class,
        dpv-owl:RiskConcept,
        risk-owl:PotentialConsequence,
        risk-owl:PotentialImpact,
        risk-owl:PotentialRisk ;
    dct:contributor _:N9c63c24625fe482386a350b4ea27b4f8 ;
    dct:created "2024-12-01"^^xsd:date ;
    rdfs:isDefinedBy risk-owl: ;
    rdfs:subClassOf risk-owl:HealthSafety ;
    sw:term_status "accepted"@en ;
    skos:definition "Concept representing wellbeing of individual(s)"@en ;
    skos:prefLabel "Wellbeing"@en .

risk-owl:WorkplaceDiscrimination a rdfs:Class,
        owl:Class,
        dpv-owl:RiskConcept,
        risk-owl:PotentialConsequence,
        risk-owl:PotentialImpact,
        risk-owl:PotentialRisk ;
    dct:contributor _:Ne22a67b17c7e4a779c30d2864b6a0cee ;
    dct:created "2024-12-01"^^xsd:date ;
    rdfs:isDefinedBy risk-owl: ;
    rdfs:subClassOf risk-owl:Discrimination ;
    sw:term_status "accepted"@en ;
    skos:definition "Discrimination occuring at workplace or in the context of work environments"@en ;
    skos:prefLabel "Workplace Discrimination"@en .

risk-owl:causedByThreat a rdf:Property,
        owl:ObjectProperty ;
    dcam:rangeIncludes risk-owl:Threat ;
    dct:created "2024-02-14"^^xsd:date ;
    rdfs:isDefinedBy risk-owl: ;
    sw:term_status "accepted"@en ;
    skos:definition "Indicates the cause of associated context (subject) was the indicated threat (object)"@en ;
    skos:prefLabel "caused by threat"@en ;
    schema:rangeIncludes risk-owl:Threat .

risk-owl:causedByVulnerability a rdf:Property,
        owl:ObjectProperty ;
    dcam:rangeIncludes risk-owl:Vulnerability ;
    dct:created "2024-02-14"^^xsd:date ;
    rdfs:isDefinedBy risk-owl: ;
    sw:term_status "accepted"@en ;
    skos:definition "Indicates the associated context (subject) is caused by the indicated vulnerability (object)"@en ;
    skos:prefLabel "caused by vulnerability"@en ;
    schema:rangeIncludes risk-owl:Vulnerability .

risk-owl:contains a rdf:Property,
        owl:ObjectProperty ;
    dcam:domainIncludes risk-owl:ContainmentControl ;
    dcam:rangeIncludes dpv-owl:RiskConcept ;
    dct:contributor _:Ne22a67b17c7e4a779c30d2864b6a0cee ;
    dct:created "2025-01-06"^^xsd:date ;
    rdfs:isDefinedBy risk-owl: ;
    rdfs:subPropertyOf risk-owl:controls ;
    sw:term_status "accepted"@en ;
    skos:definition "Indicates the specified event or action is contained by this control"@en ;
    skos:prefLabel "contains"@en ;
    schema:domainIncludes risk-owl:ContainmentControl ;
    schema:rangeIncludes dpv-owl:RiskConcept .

risk-owl:detects a rdf:Property,
        owl:ObjectProperty ;
    dcam:domainIncludes risk-owl:DetectionControl ;
    dcam:rangeIncludes dpv-owl:RiskConcept ;
    dct:contributor _:N9c63c24625fe482386a350b4ea27b4f8,
        _:Ne22a67b17c7e4a779c30d2864b6a0cee ;
    dct:created "2024-12-01"^^xsd:date ;
    dct:modified "2025-01-06"^^xsd:date ;
    rdfs:isDefinedBy risk-owl: ;
    rdfs:subPropertyOf risk-owl:monitors ;
    sw:term_status "modified"@en ;
    skos:definition "Indicates the specified event or action is detected by this control"@en ;
    skos:prefLabel "detects"@en ;
    schema:domainIncludes risk-owl:DetectionControl ;
    schema:rangeIncludes dpv-owl:RiskConcept .

risk-owl:eliminates a rdf:Property,
        owl:ObjectProperty ;
    dcam:domainIncludes risk-owl:EliminationControl ;
    dcam:rangeIncludes dpv-owl:RiskConcept ;
    dct:contributor _:N9c63c24625fe482386a350b4ea27b4f8,
        _:Ne22a67b17c7e4a779c30d2864b6a0cee ;
    dct:created "2024-12-01"^^xsd:date ;
    dct:modified "2025-01-06"^^xsd:date ;
    rdfs:isDefinedBy risk-owl: ;
    rdfs:subPropertyOf risk-owl:avoids ;
    sw:term_status "modified"@en ;
    skos:definition "Indicates the specified event or action is eliminated by this control"@en ;
    skos:prefLabel "eliminates"@en ;
    schema:domainIncludes risk-owl:EliminationControl ;
    schema:rangeIncludes dpv-owl:RiskConcept .

risk-owl:exploitsVulnerability a rdf:Property,
        owl:ObjectProperty ;
    dcam:domainIncludes risk-owl:Threat ;
    dcam:rangeIncludes risk-owl:Vulnerability ;
    dct:created "2024-02-14"^^xsd:date ;
    rdfs:isDefinedBy risk-owl: ;
    sw:term_status "accepted"@en ;
    skos:definition "Indicates the threat (subject) exploits the indicated vulnerability (object)"@en ;
    skos:prefLabel "exploits vulnerability"@en ;
    schema:domainIncludes risk-owl:Threat ;
    schema:rangeIncludes risk-owl:Vulnerability .

risk-owl:hasControl a rdf:Property,
        owl:ObjectProperty ;
    dcam:rangeIncludes risk-owl:RiskControl ;
    dct:contributor _:Ne22a67b17c7e4a779c30d2864b6a0cee ;
    dct:created "2024-02-14"^^xsd:date ;
    dct:modified "2025-01-06"^^xsd:date ;
    vann:example dex-owl:E0071 ;
    rdfs:isDefinedBy risk-owl: ;
    sw:term_status "modified"@en ;
    skos:definition "Indicates the use of specified control"@en ;
    skos:prefLabel "has control"@en ;
    schema:rangeIncludes risk-owl:RiskControl .

risk-owl:hasIncident a rdf:Property,
        owl:ObjectProperty ;
    dcam:rangeIncludes risk-owl:Incident ;
    dct:created "2024-02-14"^^xsd:date ;
    rdfs:isDefinedBy risk-owl: ;
    sw:term_status "accepted"@en ;
    skos:definition "Indicates an incident is associated with the specified context"@en ;
    skos:prefLabel "has incident"@en ;
    schema:rangeIncludes risk-owl:Incident .

risk-owl:hasRiskAcceptance a rdf:Property,
        owl:ObjectProperty ;
    dcam:rangeIncludes risk-owl:RiskAcceptance ;
    dct:created "2024-12-01"^^xsd:date ;
    rdfs:isDefinedBy risk-owl: ;
    sw:term_status "accepted"@en ;
    skos:definition "Associates the risk acceptance plan or process or criteria"@en ;
    skos:prefLabel "has risk acceptance"@en ;
    schema:rangeIncludes risk-owl:RiskAcceptance .

risk-owl:hasRiskAnalysis a rdf:Property,
        owl:ObjectProperty ;
    dcam:rangeIncludes risk-owl:RiskAnalysis ;
    dct:created "2024-12-01"^^xsd:date ;
    rdfs:isDefinedBy risk-owl: ;
    sw:term_status "accepted"@en ;
    skos:definition "Associates the risk analysis"@en ;
    skos:prefLabel "has risk analysis"@en ;
    schema:rangeIncludes risk-owl:RiskAnalysis .

risk-owl:hasRiskAssessment a rdf:Property,
        owl:ObjectProperty ;
    dcam:rangeIncludes risk-owl:RiskAssessment ;
    dct:created "2024-12-01"^^xsd:date ;
    rdfs:isDefinedBy risk-owl: ;
    sw:term_status "accepted"@en ;
    skos:definition "Associates the risk assessment"@en ;
    skos:prefLabel "has risk assessment"@en ;
    schema:rangeIncludes risk-owl:RiskAssessment .

risk-owl:hasRiskCriteria a rdf:Property,
        owl:ObjectProperty ;
    dcam:rangeIncludes risk-owl:RiskCriteria ;
    dct:created "2024-12-01"^^xsd:date ;
    rdfs:isDefinedBy risk-owl: ;
    sw:term_status "accepted"@en ;
    skos:definition "Associates the risk criteria"@en ;
    skos:prefLabel "has risk criteria"@en ;
    schema:rangeIncludes risk-owl:RiskCriteria .

risk-owl:hasRiskEvaluation a rdf:Property,
        owl:ObjectProperty ;
    dcam:rangeIncludes risk-owl:RiskEvaluation ;
    dct:created "2024-12-01"^^xsd:date ;
    rdfs:isDefinedBy risk-owl: ;
    sw:term_status "accepted"@en ;
    skos:definition "Associates the risk evaluation plan or process or criteria"@en ;
    skos:prefLabel "has risk evaluation"@en ;
    schema:rangeIncludes risk-owl:RiskEvaluation .

risk-owl:hasRiskIdentification a rdf:Property,
        owl:ObjectProperty ;
    dcam:rangeIncludes risk-owl:RiskIdentification ;
    dct:created "2024-12-01"^^xsd:date ;
    rdfs:isDefinedBy risk-owl: ;
    sw:term_status "accepted"@en ;
    skos:definition "Associates the risk identification plan or process or criteria"@en ;
    skos:prefLabel "has risk identification"@en ;
    schema:rangeIncludes risk-owl:RiskIdentification .

risk-owl:hasRiskManagement a rdf:Property,
        owl:ObjectProperty ;
    dcam:rangeIncludes risk-owl:RiskManagement ;
    dct:created "2024-12-01"^^xsd:date ;
    rdfs:isDefinedBy risk-owl: ;
    sw:term_status "accepted"@en ;
    skos:definition "Associates the risk management plan or process"@en ;
    skos:prefLabel "has risk management"@en ;
    schema:rangeIncludes risk-owl:RiskManagement .

risk-owl:hasRiskOwner a rdf:Property,
        owl:ObjectProperty ;
    dcam:rangeIncludes risk-owl:RiskOwner ;
    dct:created "2024-12-01"^^xsd:date ;
    rdfs:isDefinedBy risk-owl: ;
    sw:term_status "accepted"@en ;
    skos:definition "Indicates the risk owner"@en ;
    skos:prefLabel "has risk owner"@en ;
    schema:rangeIncludes risk-owl:RiskOwner .

risk-owl:hasRiskPerception a rdf:Property,
        owl:ObjectProperty ;
    dcam:rangeIncludes risk-owl:RiskPerception ;
    dct:created "2024-12-01"^^xsd:date ;
    rdfs:isDefinedBy risk-owl: ;
    sw:term_status "accepted"@en ;
    skos:definition "Associates the risk perception plan or process or criteria"@en ;
    skos:prefLabel "has risk perception"@en ;
    schema:rangeIncludes risk-owl:RiskPerception .

risk-owl:hasRiskSource a rdf:Property,
        owl:ObjectProperty ;
    dcam:domainIncludes dpv-owl:Risk ;
    dcam:rangeIncludes risk-owl:RiskSource ;
    dct:created "2024-02-14"^^xsd:date ;
    rdfs:isDefinedBy risk-owl: ;
    sw:term_status "accepted"@en ;
    skos:definition "Indicates the risk (subject) has the indicated risk source (object)"@en ;
    skos:prefLabel "has risk source"@en ;
    schema:domainIncludes dpv-owl:Risk ;
    schema:rangeIncludes risk-owl:RiskSource .

risk-owl:hasRiskTreatment a rdf:Property,
        owl:ObjectProperty ;
    dcam:rangeIncludes risk-owl:RiskTreatment ;
    dct:created "2024-12-01"^^xsd:date ;
    rdfs:isDefinedBy risk-owl: ;
    sw:term_status "accepted"@en ;
    skos:definition "Associates the risk treatment plan or process or criteria"@en ;
    skos:prefLabel "has risk treatment"@en ;
    schema:rangeIncludes risk-owl:RiskTreatment .

risk-owl:hasThreatSource a rdf:Property,
        owl:ObjectProperty ;
    dcam:domainIncludes risk-owl:Threat ;
    dcam:rangeIncludes risk-owl:ThreatSource ;
    dct:created "2024-02-14"^^xsd:date ;
    rdfs:isDefinedBy risk-owl: ;
    sw:term_status "accepted"@en ;
    skos:definition "Indicates the threat (subject) has the indicated source (object)"@en ;
    skos:prefLabel "has threat source"@en ;
    schema:domainIncludes risk-owl:Threat ;
    schema:rangeIncludes risk-owl:ThreatSource .

risk-owl:hasVulnerability a rdf:Property,
        owl:ObjectProperty ;
    dcam:rangeIncludes risk-owl:Vulnerability ;
    dct:created "2024-02-14"^^xsd:date ;
    rdfs:isDefinedBy risk-owl: ;
    sw:term_status "accepted"@en ;
    skos:definition "Indicates the associated context (subject) has indicated vulnerability (object)"@en ;
    skos:prefLabel "has vulnerability"@en ;
    schema:rangeIncludes risk-owl:Vulnerability .

risk-owl:identifies a rdf:Property,
        owl:ObjectProperty ;
    dcam:domainIncludes risk-owl:IdentificationControl ;
    dcam:rangeIncludes dpv-owl:RiskConcept ;
    dct:contributor _:N9c63c24625fe482386a350b4ea27b4f8,
        _:Ne22a67b17c7e4a779c30d2864b6a0cee ;
    dct:created "2024-12-01"^^xsd:date ;
    dct:modified "2025-01-06"^^xsd:date ;
    rdfs:isDefinedBy risk-owl: ;
    rdfs:subPropertyOf risk-owl:monitors ;
    sw:term_status "modified"@en ;
    skos:definition "Indicates the specified event or action is identified by this control"@en ;
    skos:prefLabel "identifies"@en ;
    schema:domainIncludes risk-owl:IdentificationControl ;
    schema:rangeIncludes dpv-owl:RiskConcept .

risk-owl:interrupts a rdf:Property,
        owl:ObjectProperty ;
    dcam:domainIncludes risk-owl:InterruptionControl ;
    dcam:rangeIncludes dpv-owl:RiskConcept ;
    dct:contributor _:Ne22a67b17c7e4a779c30d2864b6a0cee ;
    dct:created "2025-01-06"^^xsd:date ;
    rdfs:isDefinedBy risk-owl: ;
    rdfs:subPropertyOf risk-owl:reduces ;
    sw:term_status "accepted"@en ;
    skos:definition "Indicates the specified event or action is interrupted by this control"@en ;
    skos:prefLabel "interrupts"@en ;
    schema:domainIncludes risk-owl:InterruptionControl ;
    schema:rangeIncludes dpv-owl:RiskConcept .

risk-owl:intervenes a rdf:Property,
        owl:ObjectProperty ;
    dcam:domainIncludes risk-owl:InterventionControl ;
    dcam:rangeIncludes dpv-owl:RiskConcept ;
    dct:contributor _:Ne22a67b17c7e4a779c30d2864b6a0cee ;
    dct:created "2025-01-06"^^xsd:date ;
    rdfs:isDefinedBy risk-owl: ;
    rdfs:subPropertyOf risk-owl:reduces ;
    sw:term_status "accepted"@en ;
    skos:definition "Indicates the specified event or action is intervened by this control"@en ;
    skos:prefLabel "intervenes"@en ;
    schema:domainIncludes risk-owl:InterventionControl ;
    schema:rangeIncludes dpv-owl:RiskConcept .

risk-owl:investigates a rdf:Property,
        owl:ObjectProperty ;
    dcam:domainIncludes risk-owl:InvestigationControl ;
    dcam:rangeIncludes dpv-owl:RiskConcept ;
    dct:contributor _:Ne22a67b17c7e4a779c30d2864b6a0cee ;
    dct:created "2025-01-06"^^xsd:date ;
    rdfs:isDefinedBy risk-owl: ;
    rdfs:subPropertyOf risk-owl:controls ;
    sw:term_status "accepted"@en ;
    skos:definition "Indicates the specified event or action is investigated by this control"@en ;
    skos:prefLabel "investigates"@en ;
    schema:domainIncludes risk-owl:InvestigationControl ;
    schema:rangeIncludes dpv-owl:RiskConcept .

risk-owl:isExploitedBy a rdf:Property,
        owl:ObjectProperty ;
    dcam:domainIncludes risk-owl:Vulnerability ;
    dcam:rangeIncludes risk-owl:Threat ;
    dct:created "2024-02-14"^^xsd:date ;
    rdfs:isDefinedBy risk-owl: ;
    sw:term_status "accepted"@en ;
    skos:definition "Indicates the vulnerability (subject) is exploited by the indicated threat (object)"@en ;
    skos:prefLabel "is exploited by"@en ;
    schema:domainIncludes risk-owl:Vulnerability ;
    schema:rangeIncludes risk-owl:Threat .

risk-owl:isVulnerabilityOf a rdf:Property,
        owl:ObjectProperty ;
    dcam:domainIncludes risk-owl:Vulnerability ;
    dct:created "2024-02-14"^^xsd:date ;
    rdfs:isDefinedBy risk-owl: ;
    sw:term_status "accepted"@en ;
    skos:definition "Indicates the vulnerability (subject) is associated with indicated context (object)"@en ;
    skos:prefLabel "is vulnerability of"@en ;
    schema:domainIncludes risk-owl:Vulnerability .

risk-owl:logs a rdf:Property,
        owl:ObjectProperty ;
    dcam:domainIncludes risk-owl:LoggingControl ;
    dcam:rangeIncludes dpv-owl:RiskConcept ;
    dct:contributor _:Ne22a67b17c7e4a779c30d2864b6a0cee ;
    dct:created "2025-01-06"^^xsd:date ;
    rdfs:isDefinedBy risk-owl: ;
    rdfs:subPropertyOf risk-owl:monitors ;
    sw:term_status "accepted"@en ;
    skos:definition "Indicates the specified event or action is logged by this control"@en ;
    skos:prefLabel "logs"@en ;
    schema:domainIncludes risk-owl:LoggingControl ;
    schema:rangeIncludes dpv-owl:RiskConcept .

risk-owl:mitigates a rdf:Property,
        owl:ObjectProperty ;
    dcam:domainIncludes risk-owl:MitigationControl ;
    dcam:rangeIncludes dpv-owl:RiskConcept ;
    dct:contributor _:N9c63c24625fe482386a350b4ea27b4f8,
        _:Ne22a67b17c7e4a779c30d2864b6a0cee ;
    dct:created "2024-12-01"^^xsd:date ;
    dct:modified "2025-01-06"^^xsd:date ;
    rdfs:isDefinedBy risk-owl: ;
    rdfs:subPropertyOf risk-owl:avoids ;
    sw:term_status "modified"@en ;
    skos:definition "Indicates the specified event or action is mitigated by this control"@en ;
    skos:prefLabel "mitigates"@en ;
    schema:domainIncludes risk-owl:MitigationControl ;
    schema:rangeIncludes dpv-owl:RiskConcept .

risk-owl:modifies a rdf:Property,
        owl:ObjectProperty ;
    dcam:domainIncludes risk-owl:ModificationControl ;
    dcam:rangeIncludes dpv-owl:RiskConcept ;
    dct:contributor _:N9c63c24625fe482386a350b4ea27b4f8,
        _:Ne22a67b17c7e4a779c30d2864b6a0cee ;
    dct:created "2024-12-01"^^xsd:date ;
    dct:modified "2025-01-06"^^xsd:date ;
    rdfs:isDefinedBy risk-owl: ;
    rdfs:subPropertyOf risk-owl:avoids ;
    sw:term_status "modified"@en ;
    skos:definition "Indicates the specified event or action is modified by this control"@en ;
    skos:prefLabel "modifies"@en ;
    schema:domainIncludes risk-owl:ModificationControl ;
    schema:rangeIncludes dpv-owl:RiskConcept .

risk-owl:overrides a rdf:Property,
        owl:ObjectProperty ;
    dcam:domainIncludes risk-owl:OverrideControl ;
    dcam:rangeIncludes dpv-owl:RiskConcept ;
    dct:contributor _:Ne22a67b17c7e4a779c30d2864b6a0cee ;
    dct:created "2025-01-06"^^xsd:date ;
    rdfs:isDefinedBy risk-owl: ;
    rdfs:subPropertyOf risk-owl:controls ;
    sw:term_status "accepted"@en ;
    skos:definition "Indicates the specified event or action is overridden by this control"@en ;
    skos:prefLabel "overrides"@en ;
    schema:domainIncludes risk-owl:OverrideControl ;
    schema:rangeIncludes dpv-owl:RiskConcept .

risk-owl:recovers a rdf:Property,
        owl:ObjectProperty ;
    dcam:domainIncludes risk-owl:RecoveryControl ;
    dcam:rangeIncludes dpv-owl:RiskConcept ;
    dct:contributor _:Ne22a67b17c7e4a779c30d2864b6a0cee ;
    dct:created "2025-01-06"^^xsd:date ;
    rdfs:isDefinedBy risk-owl: ;
    rdfs:subPropertyOf risk-owl:resolves ;
    sw:term_status "accepted"@en ;
    skos:definition "Indicates the specified event or action is recovered from by this control"@en ;
    skos:prefLabel "recovers"@en ;
    schema:domainIncludes risk-owl:RecoveryControl ;
    schema:rangeIncludes dpv-owl:RiskConcept .

risk-owl:refersToRisk a rdf:Property,
        owl:ObjectProperty ;
    dcam:domainIncludes dpv-owl:Incident ;
    dcam:rangeIncludes dpv-owl:Risk ;
    dct:created "2024-02-14"^^xsd:date ;
    vann:example dex-owl:E0069 ;
    rdfs:isDefinedBy risk-owl: ;
    sw:term_status "accepted"@en ;
    skos:definition "Indicates the incident (subject) is a materialisation of the indicated risk (object)"@en ;
    skos:prefLabel "refers to risk"@en ;
    schema:domainIncludes dpv-owl:Incident ;
    schema:rangeIncludes dpv-owl:Risk .

risk-owl:remedies a rdf:Property,
        owl:ObjectProperty ;
    dcam:domainIncludes risk-owl:RemediationControl ;
    dcam:rangeIncludes dpv-owl:RiskConcept ;
    dct:contributor _:Ne22a67b17c7e4a779c30d2864b6a0cee ;
    dct:created "2025-01-06"^^xsd:date ;
    rdfs:isDefinedBy risk-owl: ;
    rdfs:subPropertyOf risk-owl:resolves ;
    sw:term_status "accepted"@en ;
    skos:definition "Indicates the specified event or action is remedied by this control"@en ;
    skos:prefLabel "remedies"@en ;
    schema:domainIncludes risk-owl:RemediationControl ;
    schema:rangeIncludes dpv-owl:RiskConcept .

risk-owl:reverses a rdf:Property,
        owl:ObjectProperty ;
    dcam:domainIncludes risk-owl:ReversalControl ;
    dcam:rangeIncludes dpv-owl:RiskConcept ;
    dct:contributor _:Ne22a67b17c7e4a779c30d2864b6a0cee ;
    dct:created "2025-01-06"^^xsd:date ;
    rdfs:isDefinedBy risk-owl: ;
    rdfs:subPropertyOf risk-owl:resolves ;
    sw:term_status "accepted"@en ;
    skos:definition "Indicates the specified event or action is reversed by this control"@en ;
    skos:prefLabel "reverses"@en ;
    schema:domainIncludes risk-owl:ReversalControl ;
    schema:rangeIncludes dpv-owl:RiskConcept .

risk-owl:shares a rdf:Property,
        owl:ObjectProperty ;
    dcam:domainIncludes risk-owl:ShareControl ;
    dcam:rangeIncludes dpv-owl:RiskConcept ;
    dct:contributor _:Ne22a67b17c7e4a779c30d2864b6a0cee ;
    dct:created "2025-01-06"^^xsd:date ;
    rdfs:isDefinedBy risk-owl: ;
    rdfs:subPropertyOf risk-owl:controls ;
    sw:term_status "accepted"@en ;
    skos:definition "Indicates the specified event or action is shared with another context or entity by this control"@en ;
    skos:prefLabel "shares"@en ;
    schema:domainIncludes risk-owl:ShareControl ;
    schema:rangeIncludes dpv-owl:RiskConcept .

risk-owl:substitutes a rdf:Property,
        owl:ObjectProperty ;
    dcam:domainIncludes risk-owl:SubstitutionControl ;
    dcam:rangeIncludes dpv-owl:RiskConcept ;
    dct:contributor _:Ne22a67b17c7e4a779c30d2864b6a0cee ;
    dct:created "2025-01-06"^^xsd:date ;
    rdfs:isDefinedBy risk-owl: ;
    rdfs:subPropertyOf risk-owl:avoids ;
    sw:term_status "accepted"@en ;
    skos:definition "Indicates the specified event or action is substituted by this control"@en ;
    skos:prefLabel "substitutes"@en ;
    schema:domainIncludes risk-owl:SubstitutionControl ;
    schema:rangeIncludes dpv-owl:RiskConcept .

risk-owl:transfers a rdf:Property,
        owl:ObjectProperty ;
    dcam:domainIncludes risk-owl:TransferControl ;
    dcam:rangeIncludes dpv-owl:RiskConcept ;
    dct:contributor _:Ne22a67b17c7e4a779c30d2864b6a0cee ;
    dct:created "2025-01-06"^^xsd:date ;
    rdfs:isDefinedBy risk-owl: ;
    rdfs:subPropertyOf risk-owl:controls ;
    sw:term_status "accepted"@en ;
    skos:definition "Indicates the specified event or action is transfered to another context or entity by this control"@en ;
    skos:prefLabel "transfers"@en ;
    schema:domainIncludes risk-owl:TransferControl ;
    schema:rangeIncludes dpv-owl:RiskConcept .

risk-owl:serialisation-html a profile:ResourceDescriptor ;
    dct:conformsTo <https://www.w3.org/TR/html/> ;
    dct:format <https://www.iana.org/assignments/media-types/text/html> ;
    dct:title "Risk Concepts - HTML serialiation" ;
    profile:hasArtifact <https://w3id.org/dpv/risk/risk-owl.html> ;
    profile:hasRole role:specification .

risk-owl:serialisation-jsonld a profile:ResourceDescriptor ;
    dct:conformsTo <https://www.w3.org/TR/json-ld11/> ;
    dct:format <https://www.iana.org/assignments/media-types/application/ld+json> ;
    dct:title "Risk Concepts - JSON-LD serialiation" ;
    profile:hasArtifact <https://w3id.org/dpv/risk/risk-owl.jsonld> ;
    profile:hasRole role:vocabulary .

risk-owl:serialisation-n3 a profile:ResourceDescriptor ;
    dct:conformsTo <https://www.w3.org/TeamSubmission/n3/> ;
    dct:format <https://www.iana.org/assignments/media-types/text/n3> ;
    dct:title "Risk Concepts - N3 serialiation" ;
    profile:hasArtifact <https://w3id.org/dpv/risk/risk-owl.n3> ;
    profile:hasRole role:vocabulary .

risk-owl:serialisation-rdf a profile:ResourceDescriptor ;
    dct:conformsTo rdf: ;
    dct:format <https://www.iana.org/assignments/media-types/application/rdf+xml> ;
    dct:title "Risk Concepts - RDF/XML serialiation" ;
    profile:hasArtifact <https://w3id.org/dpv/risk/risk-owl.rdf> ;
    profile:hasRole role:vocabulary .

risk-owl:serialisation-ttl a profile:ResourceDescriptor ;
    dct:conformsTo <https://www.w3.org/TR/turtle/> ;
    dct:format <https://www.iana.org/assignments/media-types/text/turtle> ;
    dct:title "Risk Concepts - Turtle serialiation" ;
    profile:hasArtifact <https://w3id.org/dpv/risk/risk-owl.ttl> ;
    profile:hasRole role:vocabulary .

<https://w3id.org/dpv/examples> a profile:ResourceDescriptor ;
    dct:conformsTo <https://www.w3.org/TR/html/> ;
    dct:format <https://www.iana.org/assignments/media-types/text/html> ;
    dct:title "Examples for Data Privacy Vocabulary" ;
    profile:hasArtifact <https://w3id.org/dpv/examples> ;
    profile:hasRole role:guidance .

<https://w3id.org/dpv/guides> a profile:ResourceDescriptor ;
    dct:conformsTo <https://www.w3.org/TR/html/> ;
    dct:format <https://www.iana.org/assignments/media-types/text/html> ;
    dct:title "Guides for Data Privacy Vocabulary" ;
    profile:hasArtifact <https://w3id.org/dpv/guides> ;
    profile:hasRole role:guidance .

<https://w3id.org/dpv/primer> a profile:ResourceDescriptor ;
    dct:conformsTo <https://www.w3.org/TR/html/> ;
    dct:format <https://www.iana.org/assignments/media-types/text/html> ;
    dct:title "Primer for Data Privacy Vocabulary" ;
    profile:hasArtifact <https://w3id.org/dpv/primer> ;
    profile:hasRole role:guidance .

risk-owl:monitors a rdf:Property,
        owl:ObjectProperty ;
    dcam:domainIncludes risk-owl:MonitorControl ;
    dcam:rangeIncludes dpv-owl:RiskConcept ;
    dct:contributor _:Ne22a67b17c7e4a779c30d2864b6a0cee ;
    dct:created "2025-01-06"^^xsd:date ;
    rdfs:isDefinedBy risk-owl: ;
    rdfs:subPropertyOf risk-owl:controls ;
    sw:term_status "accepted"@en ;
    skos:definition "Indicates the specified event or action is monitored by this control"@en ;
    skos:prefLabel "monitors"@en ;
    schema:domainIncludes risk-owl:MonitorControl ;
    schema:rangeIncludes dpv-owl:RiskConcept .

risk-owl:reduces a rdf:Property,
        owl:ObjectProperty ;
    dcam:domainIncludes risk-owl:ReductionControl ;
    dcam:rangeIncludes dpv-owl:RiskConcept ;
    dct:contributor _:Ne22a67b17c7e4a779c30d2864b6a0cee ;
    dct:created "2025-01-06"^^xsd:date ;
    rdfs:isDefinedBy risk-owl: ;
    rdfs:subPropertyOf risk-owl:controls ;
    sw:term_status "accepted"@en ;
    skos:definition "Indicates the specified event or action is reduced by this control"@en ;
    skos:prefLabel "reduces"@en ;
    schema:domainIncludes risk-owl:ReductionControl ;
    schema:rangeIncludes dpv-owl:RiskConcept .

risk-owl:resolves a rdf:Property,
        owl:ObjectProperty ;
    dcam:domainIncludes risk-owl:ResolutionControl ;
    dcam:rangeIncludes dpv-owl:RiskConcept ;
    dct:contributor _:Ne22a67b17c7e4a779c30d2864b6a0cee ;
    dct:created "2025-01-06"^^xsd:date ;
    rdfs:isDefinedBy risk-owl: ;
    rdfs:subPropertyOf risk-owl:controls ;
    sw:term_status "accepted"@en ;
    skos:definition "Indicates the specified event or action is resolved by this control"@en ;
    skos:prefLabel "resolves"@en ;
    schema:domainIncludes risk-owl:ResolutionControl ;
    schema:rangeIncludes dpv-owl:RiskConcept .

risk-owl:avoids a rdf:Property,
        owl:ObjectProperty ;
    dcam:domainIncludes risk-owl:AvoidanceControl ;
    dcam:rangeIncludes dpv-owl:RiskConcept ;
    dct:contributor _:Ne22a67b17c7e4a779c30d2864b6a0cee ;
    dct:created "2025-01-06"^^xsd:date ;
    rdfs:isDefinedBy risk-owl: ;
    rdfs:subPropertyOf risk-owl:reduces ;
    sw:term_status "accepted"@en ;
    skos:definition "Indicates the event or action is avoided by the specified control"@en ;
    skos:prefLabel "avoids"@en ;
    schema:domainIncludes risk-owl:AvoidanceControl ;
    schema:rangeIncludes dpv-owl:RiskConcept .

risk-owl:controls a rdf:Property,
        owl:ObjectProperty ;
    dcam:domainIncludes risk-owl:RiskControl ;
    dcam:rangeIncludes dpv-owl:RiskConcept ;
    dct:contributor _:Ne22a67b17c7e4a779c30d2864b6a0cee ;
    dct:created "2025-01-06"^^xsd:date ;
    vann:example dex-owl:E0086 ;
    rdfs:isDefinedBy risk-owl: ;
    sw:term_status "accepted"@en ;
    skos:definition "Indicates this control manages specified risk concept event or action, such as for risk sources, risks, consequences, and impacts"@en ;
    skos:prefLabel "control"@en ;
    schema:domainIncludes risk-owl:RiskControl ;
    schema:rangeIncludes dpv-owl:RiskConcept .

risk-owl: a owl:Ontology,
        profile:Profile ;
    dct:bibliographicCitation "Harshvardhan J. Pandit, Beatriz Esteves, Georg P. Krog, Paul Ryan, Delaram Golpayegani, Julian Flake (2025) Data Privacy Vocabulary (DPV)  Version 2.0. In: Demartini, G., et al. The Semantic Web  ISWC 2024. ISWC 2024. Lecture Notes in Computer Science, vol 15233. Springer, Cham. https://doi.org/10.1007/978-3-031-77847-6_10" ;
    dct:conformsTo <http://www.w3.org/2002/07/owl>,
        "http://www.w3.org/2000/01/rdf-schema",
        "http://www.w3.org/2004/02/skos/core" ;
    dct:contributor _:N2e9307242cb14d528effb994db501842,
        _:N4b493e90e86f4bec907dc903aaa37183,
        _:N59852c09189e47bd989757f1615f7bdf,
        _:N75641c194b3f4973ab2abfb33aed55d3,
        _:N7d9b5ee7f31f4f2ba5951e30b49ec7c0,
        _:N9c63c24625fe482386a350b4ea27b4f8,
        _:Naa42ed8e13734cd887c18487fe7930ec,
        _:Ne22a67b17c7e4a779c30d2864b6a0cee,
        _:Ne58e82a7606b4ab9ada0b0f2f7592231,
        _:Ne84980f7db76425ca367742d2085d8c9 ;
    dct:created "2022-08-14"@en ;
    dct:creator _:N59852c09189e47bd989757f1615f7bdf,
        _:N75641c194b3f4973ab2abfb33aed55d3,
        _:N7d9b5ee7f31f4f2ba5951e30b49ec7c0,
        _:N9c63c24625fe482386a350b4ea27b4f8,
        [ a dct:Agent,
                foaf:Person ;
            scoro:hasORCID "0000-0003-0770-2737" ;
            org:memberOf [ a foaf:Organization ;
                    foaf:name "Uniphar PLC" ] ;
            foaf:name "Paul Ryan" ],
        _:Ne22a67b17c7e4a779c30d2864b6a0cee,
        _:Ne84980f7db76425ca367742d2085d8c9 ;
    dct:description "Extension to the Data Privacy Vocabulary (DPV) providing concepts for representing information about risk assessment and risk management"@en ;
    dct:hasVersion risk-owl: ;
    dct:identifier "https://w3id.org/dpv/risk" ;
    dct:issued "2022-08-14"@en ;
    dct:license <https://www.w3.org/copyright/document-license-2023/> ;
    dct:modified "2025-02-01"@en ;
    dct:publisher <https://www.w3.org/> ;
    dct:source <https://www.w3.org/groups/cg/dpvcg/> ;
    dct:title "Risk Concepts"@en ;
    bibo:doi "10.5281/zenodo.12505841" ;
    bibo:status "http://purl.org/ontology/bibo/status/published" ;
    vann:preferredNamespacePrefix "risk" ;
    vann:preferredNamespaceUri "https://w3id.org/dpv/risk#" ;
    rdfs:Label "RISK"@en ;
    owl:versionIRI <https://w3id.org/dpv/2.1/risk/owl#> ;
    owl:versionInfo "2.1" ;
    profile:hasResource <https://w3id.org/dpv/examples>,
        <https://w3id.org/dpv/guides>,
        <https://w3id.org/dpv/primer>,
        risk-owl:serialisation-html,
        risk-owl:serialisation-jsonld,
        risk-owl:serialisation-n3,
        risk-owl:serialisation-rdf,
        risk-owl:serialisation-ttl ;
    profile:isProfileOf <http://www.w3.org/2002/07/owl>,
        <https://w3id.org/dpv/owl>,
        risk-owl: ;
    foaf:logo <https://w3id.org/dpv/media/logo.png> ;
    schema:version "2.1" .

_:N0c4f26726681494f8f9054328c810c07 a foaf:Organization ;
    foaf:name "University College Dublin" .

_:N1179325f3fdc440ea7096a5f4b108a44 a foaf:Organization ;
    foaf:name "University of Koblenz" .

_:N1f3f592e60884deca0c831c0e62adabb a foaf:Organization ;
    foaf:name "Vienna University of Economics and Business" .

_:N2b218fbf49474a93a5f1d76695037221 a foaf:Organization ;
    foaf:name "ADAPT Centre, Trinity College Dublin" .

_:N420af302e4e94354ab0cbfde2188b0b4 a foaf:Organization ;
    foaf:name "Trinity College Dublin" .

_:N6cd6ef5ec58745369be45f4a23814332 a foaf:Organization ;
    foaf:name "ADAPT Centre, Dublin City University" .

_:N7c91f8fe3e644e0faad89b617c1d0581 a foaf:Organization ;
    foaf:name "Dublin City University" .

_:N93888206f03d482f86db2078dc52e4da a foaf:Organization ;
    foaf:name "Signatu AS" .

_:Na3cb797dfb7342b792beed15c9fe3b1a a foaf:Organization ;
    foaf:name "Vienna University of Technology" .

_:Nb10f7ca597f946ef8f976f1681fc0421 a foaf:Organization ;
    foaf:name "IDLab, IMEC, Ghent University" .

_:Naa42ed8e13734cd887c18487fe7930ec a dct:Agent,
        foaf:Person ;
    org:memberOf _:N7c91f8fe3e644e0faad89b617c1d0581 ;
    foaf:name "Julio Fernandez" .

_:Ne58e82a7606b4ab9ada0b0f2f7592231 a dct:Agent,
        foaf:Person ;
    org:memberOf _:N1f3f592e60884deca0c831c0e62adabb ;
    foaf:name "Axel Polleres" .

_:N4b493e90e86f4bec907dc903aaa37183 a dct:Agent,
        foaf:Person ;
    org:memberOf _:Na3cb797dfb7342b792beed15c9fe3b1a ;
    foaf:name "Fajar Ekaputra" .

_:N59852c09189e47bd989757f1615f7bdf a dct:Agent,
        foaf:Person ;
    org:memberOf _:N0c4f26726681494f8f9054328c810c07 ;
    foaf:name "Rob Brennan" .

_:N75641c194b3f4973ab2abfb33aed55d3 a dct:Agent,
        foaf:Person ;
    scoro:hasORCID "0000-0003-0259-7560" ;
    org:memberOf _:Nb10f7ca597f946ef8f976f1681fc0421 ;
    foaf:name "Beatriz Esteves" .

_:Ne84980f7db76425ca367742d2085d8c9 a dct:Agent,
        foaf:Person ;
    scoro:hasORCID "0009-0006-4623-1463" ;
    org:memberOf _:N1179325f3fdc440ea7096a5f4b108a44 ;
    foaf:name "Julian Flake" .

_:N7d9b5ee7f31f4f2ba5951e30b49ec7c0 a dct:Agent,
        foaf:Person ;
    org:memberOf _:N93888206f03d482f86db2078dc52e4da ;
    foaf:homepage "https://www.linkedin.com/in/georg-philip-krog-a2a278104/" ;
    foaf:name "Georg P. Krog" .

_:N2e9307242cb14d528effb994db501842 a dct:Agent,
        foaf:Person ;
    org:memberOf _:N420af302e4e94354ab0cbfde2188b0b4 ;
    foaf:name "Daniel Doherty" .

_:N9c63c24625fe482386a350b4ea27b4f8 a dct:Agent,
        foaf:Person ;
    scoro:hasORCID "0000-0002-1208-186X" ;
    org:memberOf _:N2b218fbf49474a93a5f1d76695037221 ;
    foaf:name "Delaram Golpayegani" .

_:Ne22a67b17c7e4a779c30d2864b6a0cee a dct:Agent,
        foaf:Person ;
    scoro:hasORCID "0000-0002-5068-3714" ;
    org:memberOf _:N6cd6ef5ec58745369be45f4a23814332 ;
    foaf:homepage "https://harshp.com/" ;
    foaf:name "Harshvardhan J. Pandit" .

