@prefix bibo: <http://purl.org/ontology/bibo/> .
@prefix dct: <http://purl.org/dc/terms/> .
@prefix eu-aiact: <https://w3id.org/dpv/legal/eu/aiact#> .
@prefix foaf: <http://xmlns.com/foaf/0.1/> .
@prefix org: <http://www.w3.org/ns/org#> .
@prefix owl: <http://www.w3.org/2002/07/owl#> .
@prefix profile: <http://www.w3.org/ns/dx/prof/> .
@prefix rdfs: <http://www.w3.org/2000/01/rdf-schema#> .
@prefix role: <http://www.w3.org/ns/dx/prof/role/> .
@prefix schema: <https://schema.org/> .
@prefix scoro: <http://purl.org/spar/scoro/> .
@prefix skos: <http://www.w3.org/2004/02/skos/core#> .
@prefix sw: <http://www.w3.org/2003/06/sw-vocab-status/ns#> .
@prefix vann: <http://purl.org/vocab/vann/> .
@prefix xsd: <http://www.w3.org/2001/XMLSchema#> .

eu-aiact:ProhibitedAISystem-A5-1-a a rdfs:Class,
        skos:Concept,
        eu-aiact:ProhibitedAISystem ;
    dct:contributor _:person-delaram-golpayegani ;
    dct:created "2026-02-09"^^xsd:date ;
    dct:source "AIA(Art.5(1a))"@en ;
    rdfs:isDefinedBy eu-aiact: ;
    sw:term_status "accepted"@en ;
    skos:broader eu-aiact:ProhibitedAISystem ;
    skos:definition "Prohibited AI system according to Article 5(1a) of the AI Act, indicating an AI system that deploys subliminal techniques beyond a person’s consciousness or purposefully manipulative or deceptive techniques, with the objective, or the effect of materially distorting the behaviour of a person or a group of persons by appreciably impairing their ability to make an informed decision, thereby causing them to take a decision that they would not have otherwise taken in a manner that causes or is reasonably likely to cause that person, another person or group of persons significant harm."@en ;
    skos:inScheme eu-aiact:prohibited-systems-classes ;
    skos:prefLabel "Prohibited AI System - Article 5(1a)"@en ;
    eu-aiact:hasRiskLevel eu-aiact:RiskLevelProhibited .

eu-aiact:ProhibitedAISystem-A5-1-b a rdfs:Class,
        skos:Concept,
        eu-aiact:ProhibitedAISystem ;
    dct:contributor _:person-delaram-golpayegani ;
    dct:created "2026-02-09"^^xsd:date ;
    dct:source "AIA(Art.5(1b))"@en ;
    rdfs:isDefinedBy eu-aiact: ;
    sw:term_status "accepted"@en ;
    skos:broader eu-aiact:ProhibitedAISystem ;
    skos:definition "Prohibited AI system according to Article 5(1b) of the AI Act, indicating an AI system that exploits any of the vulnerabilities of a natural person or a specific group of persons due to their age, disability or a specific social or economic situation, with the objective, or the effect, of materially distorting the behaviour of that person or a person belonging to that group in a manner that causes or is reasonably likely to cause that person or another person significant harm."@en ;
    skos:inScheme eu-aiact:prohibited-systems-classes ;
    skos:prefLabel "Prohibited AI System - Article 5(1b)"@en ;
    eu-aiact:hasRiskLevel eu-aiact:RiskLevelProhibited .

eu-aiact:ProhibitedAISystem-A5-1-c a rdfs:Class,
        skos:Concept,
        eu-aiact:ProhibitedAISystem ;
    dct:contributor _:person-delaram-golpayegani ;
    dct:created "2026-02-09"^^xsd:date ;
    dct:source "AIA(Art.5(1c))"@en ;
    rdfs:isDefinedBy eu-aiact: ;
    sw:term_status "accepted"@en ;
    skos:broader eu-aiact:ProhibitedAISystem ;
    skos:definition "Prohibited AI system according to Article 5(1c) of the AI Act, indicating AI systems that evaluate or classify of natural persons or groups of persons over a certain period of time based on their social behaviour or known, inferred or predicted personal or personality characteristics, with the social score leading to either or both of the following:  (i) detrimental or unfavourable treatment of certain natural persons or groups of persons in social contexts that are unrelated to the contexts in which the data was originally generated or collected; (ii) detrimental or unfavourable treatment of certain natural persons or groups of persons that is unjustified or disproportionate to their social behaviour or its gravity;"@en ;
    skos:inScheme eu-aiact:prohibited-systems-classes ;
    skos:prefLabel "Prohibited AI System - Article 5(1c)"@en ;
    eu-aiact:hasRiskLevel eu-aiact:RiskLevelProhibited .

eu-aiact:ProhibitedAISystem-A5-1-d a rdfs:Class,
        skos:Concept,
        eu-aiact:ProhibitedAISystem ;
    dct:contributor _:person-delaram-golpayegani ;
    dct:created "2026-02-09"^^xsd:date ;
    dct:source "AIA(Art.5(1d))"@en ;
    rdfs:isDefinedBy eu-aiact: ;
    sw:term_status "accepted"@en ;
    skos:broader eu-aiact:ProhibitedAISystem ;
    skos:definition "Prohibited AI system according to Article 5(1d) of the AI Act, indicating AI system used for making risk assessments of natural persons in order to assess or predict the risk of a natural person committing a criminal offence, based solely on the profiling of a natural person or on assessing their personality traits and characteristics; this prohibition shall not apply to AI systems used to support the human assessment of the involvement of a person in a criminal activity, which is already based on objective and verifiable facts directly linked to a criminal activity"@en ;
    skos:inScheme eu-aiact:prohibited-systems-classes ;
    skos:prefLabel "Prohibited AI System -  Article 5(1d)"@en ;
    eu-aiact:hasRiskLevel eu-aiact:RiskLevelProhibited .

eu-aiact:ProhibitedAISystem-A5-1-e a rdfs:Class,
        skos:Concept,
        eu-aiact:ProhibitedAISystem ;
    dct:contributor _:person-delaram-golpayegani ;
    dct:created "2026-02-09"^^xsd:date ;
    dct:source "AIA(Art.5(1e))"@en ;
    rdfs:isDefinedBy eu-aiact: ;
    sw:term_status "accepted"@en ;
    skos:broader eu-aiact:ProhibitedAISystem ;
    skos:definition "Prohibited AI system according to Article 5(1e) of the AI Act, indicating AI systems that create or expand facial recognition databases through the untargeted scraping of facial images from the internet or CCTV footage"@en ;
    skos:inScheme eu-aiact:prohibited-systems-classes ;
    skos:prefLabel "Prohibited AI System - Article 5(1e)"@en ;
    eu-aiact:hasRiskLevel eu-aiact:RiskLevelProhibited .

eu-aiact:ProhibitedAISystem-A5-1-f a rdfs:Class,
        skos:Concept,
        eu-aiact:ProhibitedAISystem ;
    dct:contributor _:person-delaram-golpayegani ;
    dct:created "2026-02-09"^^xsd:date ;
    dct:source "AIA(Art.5(1f))"@en ;
    rdfs:isDefinedBy eu-aiact: ;
    sw:term_status "accepted"@en ;
    skos:broader eu-aiact:ProhibitedAISystem ;
    skos:definition """Prohibited AI system according to Article 5(1f) of the AI Act, indicating  AI systems that infer emotions of a natural person in the areas of workplace and education institutions, except where the use of the AI system is
intended to be put in place or into the market for medical or safety reasons"""@en ;
    skos:inScheme eu-aiact:prohibited-systems-classes ;
    skos:prefLabel "Prohibited AI System - Article 5(1f)"@en ;
    eu-aiact:hasRiskLevel eu-aiact:RiskLevelProhibited .

eu-aiact:ProhibitedAISystem-A5-1-g a rdfs:Class,
        skos:Concept,
        eu-aiact:ProhibitedAISystem ;
    dct:contributor _:person-delaram-golpayegani ;
    dct:created "2026-02-09"^^xsd:date ;
    dct:source "AIA(Art.5(1g))"@en ;
    rdfs:isDefinedBy eu-aiact: ;
    sw:term_status "accepted"@en ;
    skos:broader eu-aiact:ProhibitedAISystem ;
    skos:definition """Prohibited AI system / risk level according to Article 5(1g) of the AI Act, indicating biometric categorisation systems that categorise individually natural persons based on their biometric data to deduce or infer their race, political
opinions, trade union membership, religious or philosophical beliefs, sex life or sexual orientation; this prohibition does
not cover any labelling or filtering of lawfully acquired biometric datasets, such as images, based on biometric data or
categorizing of biometric data in the area of law enforcement."""@en ;
    skos:inScheme eu-aiact:prohibited-systems-classes ;
    skos:prefLabel "Prohibited AI System - Article 5(1g)"@en ;
    eu-aiact:hasRiskLevel eu-aiact:RiskLevelProhibited .

eu-aiact:ProhibitedAISystem-A5-1-h a rdfs:Class,
        skos:Concept,
        eu-aiact:ProhibitedAISystem ;
    dct:contributor _:person-delaram-golpayegani ;
    dct:created "2026-02-09"^^xsd:date ;
    dct:source "AIA(Art.5(1h))"@en ;
    rdfs:isDefinedBy eu-aiact: ;
    sw:term_status "accepted"@en ;
    skos:broader eu-aiact:ProhibitedAISystem ;
    skos:definition """Prohibited AI system according to Article 5(1h) of the AI Act,  the use of ‘real-time’ remote biometric identification systems in publicly accessible spaces for the purposes of law enforcement, unless and in so far as such use is strictly necessary for one of the following objectives:
(i) the targeted search for specific victims of abduction, trafficking in human beings or sexual exploitation of human
beings, as well as the search for missing persons;
(ii) the prevention of a specific, substantial and imminent threat to the life or physical safety of natural persons or
a genuine and present or genuine and foreseeable threat of a terrorist attack;
(iii) the localisation or identification of a person suspected of having committed a criminal offence, for the purpose of
conducting a criminal investigation or prosecution or executing a criminal penalty for offences referred to in
Annex II and punishable in the Member State concerned by a custodial sentence or a detention order for
a maximum period of at least four years."""@en ;
    skos:inScheme eu-aiact:prohibited-systems-classes ;
    skos:prefLabel "Prohibited AI System - Article 5(1h)"@en ;
    eu-aiact:hasRiskLevel eu-aiact:RiskLevelProhibited .

<https://w3id.org/dpv/legal/eu/aiact> a owl:Ontology,
        profile:Profile ;
    dct:bibliographicCitation "Harshvardhan J. Pandit, Beatriz Esteves, Georg P. Krog, Paul Ryan, Delaram Golpayegani, Julian Flake (2025) Data Privacy Vocabulary (DPV) – Version 2.0. In: Demartini, G., et al. The Semantic Web – ISWC 2024. ISWC 2024. Lecture Notes in Computer Science, vol 15233. Springer, Cham. https://doi.org/10.1007/978-3-031-77847-6_10" ;
    dct:conformsTo "http://www.w3.org/2000/01/rdf-schema",
        "http://www.w3.org/2004/02/skos/core" ;
    dct:contributor _:person-delaram-golpayegani ;
    dct:created "2024-04-10"@en ;
    dct:creator _:person-delaram-golpayegani ;
    dct:description "Extension to the Data Privacy Vocabulary (DPV) providing concepts for representing information associated with EU AI Act"@en ;
    dct:identifier "https://w3id.org/dpv/legal/eu/aiact" ;
    dct:issued "2024-04-10"@en ;
    dct:license <https://www.w3.org/copyright/document-license-2023/> ;
    dct:modified "2026-02-25"@en ;
    dct:publisher <https://www.w3.org/> ;
    dct:source <https://www.w3.org/groups/cg/dpvcg/> ;
    dct:title "EU Artificial Intelligence Act (AI Act)"@en ;
    bibo:doi "10.5281/zenodo.12505841" ;
    bibo:status "http://purl.org/ontology/bibo/status/published" ;
    vann:preferredNamespacePrefix "eu-aiact" ;
    vann:preferredNamespaceUri "https://w3id.org/dpv/legal/eu/aiact#" ;
    rdfs:Label "EU-AIACT"@en ;
    owl:versionIRI <https://w3id.org/dpv/2.3/legal/eu/aiact> ;
    owl:versionInfo "2.3" ;
    profile:hasResource <https://w3id.org/dpv/examples>,
        <https://w3id.org/dpv/guides>,
        eu-aiact:serialisation-html,
        eu-aiact:serialisation-ttl,
        <https://w3id.org/dpv/primer> ;
    profile:isProfileOf rdfs:,
        skos:,
        <https://w3id.org/dpv> ;
    foaf:logo <https://w3id.org/dpv/media/logo.png> ;
    schema:version "2.3" .

eu-aiact:serialisation-html a profile:ResourceDescriptor ;
    dct:conformsTo <https://www.w3.org/TR/html/> ;
    dct:format <https://www.iana.org/assignments/media-types/text/html> ;
    dct:title "EU Artificial Intelligence Act (AI Act) - HTML serialisation" ;
    profile:hasArtifact <https://w3id.org/dpv/legal/eu/aiact/eu-aiact.html> ;
    profile:hasRole role:specification .

eu-aiact:serialisation-ttl a profile:ResourceDescriptor ;
    dct:conformsTo <https://www.w3.org/TR/turtle/> ;
    dct:format <https://www.iana.org/assignments/media-types/text/turtle> ;
    dct:title "EU Artificial Intelligence Act (AI Act) - Turtle serialisation" ;
    profile:hasArtifact <https://w3id.org/dpv/legal/eu/aiact/eu-aiact.ttl> ;
    profile:hasRole role:vocabulary .

<https://w3id.org/dpv/examples> a profile:ResourceDescriptor ;
    dct:conformsTo <https://www.w3.org/TR/html/> ;
    dct:format <https://www.iana.org/assignments/media-types/text/html> ;
    dct:title "Examples" ;
    profile:hasArtifact <https://w3id.org/dpv/examples> ;
    profile:hasRole role:guidance .

<https://w3id.org/dpv/guides> a profile:ResourceDescriptor ;
    dct:conformsTo <https://www.w3.org/TR/html/> ;
    dct:format <https://www.iana.org/assignments/media-types/text/html> ;
    dct:title "Guides for Data Privacy Vocabulary" ;
    profile:hasArtifact <https://w3id.org/dpv/guides> ;
    profile:hasRole role:guidance .

<https://w3id.org/dpv/primer> a profile:ResourceDescriptor ;
    dct:conformsTo <https://www.w3.org/TR/html/> ;
    dct:format <https://www.iana.org/assignments/media-types/text/html> ;
    dct:title "Primer for Data Privacy Vocabulary" ;
    profile:hasArtifact <https://w3id.org/dpv/primer> ;
    profile:hasRole role:guidance .

eu-aiact:prohibited-systems-classes a skos:ConceptScheme .

_:org-adapt-centre-trinity-college-dublin a foaf:Organization ;
    foaf:name "ADAPT Centre, Trinity College Dublin" .

_:person-delaram-golpayegani a dct:Agent,
        foaf:Person ;
    scoro:hasORCID "0000-0002-1208-186X" ;
    org:memberOf _:org-adapt-centre-trinity-college-dublin ;
    foaf:name "Delaram Golpayegani" .

