@prefix bibo: <http://purl.org/ontology/bibo/> .
@prefix dcam: <http://purl.org/dc/dcam/> .
@prefix dct: <http://purl.org/dc/terms/> .
@prefix dex-owl: <https://w3id.org/dpv/examples/owl#> .
@prefix dpv-owl: <https://w3id.org/dpv/owl#> .
@prefix foaf: <http://xmlns.com/foaf/0.1/> .
@prefix org: <http://www.w3.org/ns/org#> .
@prefix owl: <http://www.w3.org/2002/07/owl#> .
@prefix profile: <http://www.w3.org/ns/dx/prof/> .
@prefix rdf: <http://www.w3.org/1999/02/22-rdf-syntax-ns#> .
@prefix rdfs: <http://www.w3.org/2000/01/rdf-schema#> .
@prefix risk-owl: <https://w3id.org/dpv/risk/owl#> .
@prefix role: <http://www.w3.org/ns/dx/prof/role/> .
@prefix schema: <https://schema.org/> .
@prefix scoro: <http://purl.org/spar/scoro/> .
@prefix skos: <http://www.w3.org/2004/02/skos/core#> .
@prefix sw: <http://www.w3.org/2003/06/sw-vocab-status/ns#> .
@prefix vann: <http://purl.org/vocab/vann/> .
@prefix xsd: <http://www.w3.org/2001/XMLSchema#> .

risk-owl:RiskAcceptance a rdfs:Class,
        owl:Class ;
    dct:created "2024-12-01"^^xsd:date ;
    rdfs:isDefinedBy risk-owl: ;
    rdfs:subClassOf risk-owl:RiskManagement ;
    sw:term_status "accepted"@en ;
    skos:definition "Entity decision to accept or enable a particular risk"@en ;
    skos:prefLabel "Risk Acceptance"@en .

risk-owl:RiskAnalysis a rdfs:Class,
        owl:Class ;
    dct:contributor _:N0a43dd9ea5e94fe695d8b7df8802cfdd ;
    dct:created "2022-08-18"^^xsd:date ;
    dct:source [ a schema:WebPage ;
            schema:name "IEC 31010:2019" ;
            schema:url "https://www.iso.org/standard/72140.html" ] ;
    rdfs:isDefinedBy risk-owl: ;
    rdfs:subClassOf risk-owl:RiskAssessment ;
    sw:term_status "accepted"@en ;
    skos:definition "A technique or method used to analyse and identify risk levels, sources, likelihoods, severities, and other necessary information required to conduct risk management procedures"@en ;
    skos:prefLabel "Risk Analysis"@en .

risk-owl:RiskAssessment a rdfs:Class,
        owl:Class ;
    dct:created "2024-02-14"^^xsd:date ;
    dct:source "ISO 31073:2022 Risk management vocabulary"@en ;
    rdfs:isDefinedBy risk-owl: ;
    rdfs:subClassOf risk-owl:RiskManagement ;
    sw:term_status "accepted"@en ;
    skos:definition "Assessment of risk involving its identification, analysis, and evaluation"@en ;
    skos:prefLabel "Risk Assessment"@en .

risk-owl:RiskCriteria a rdfs:Class,
        owl:Class ;
    dct:created "2024-12-01"^^xsd:date ;
    rdfs:isDefinedBy risk-owl: ;
    rdfs:subClassOf risk-owl:RiskManagement ;
    sw:term_status "accepted"@en ;
    skos:definition "Criteria for determining or evaluating significance of risk"@en ;
    skos:prefLabel "Risk Criteria"@en .

risk-owl:RiskEvaluation a rdfs:Class,
        owl:Class ;
    dct:created "2024-12-01"^^xsd:date ;
    rdfs:isDefinedBy risk-owl: ;
    rdfs:subClassOf risk-owl:RiskAssessment ;
    sw:term_status "accepted"@en ;
    skos:definition "Process determining acceptability or tolerance of risk by comparing risk analysis outcomes against risk criteria"@en ;
    skos:prefLabel "Risk Evaluation"@en .

risk-owl:RiskIdentification a rdfs:Class,
        owl:Class ;
    dct:created "2024-12-01"^^xsd:date ;
    rdfs:isDefinedBy risk-owl: ;
    rdfs:subClassOf risk-owl:RiskAssessment ;
    sw:term_status "accepted"@en ;
    skos:definition "Identification of risks involving identification of risk sources, potential incidents, their causes, and their potential consequences"@en ;
    skos:prefLabel "Risk Identification"@en .

risk-owl:RiskManagement a rdfs:Class,
        owl:Class ;
    dct:created "2024-06-12"^^xsd:date ;
    dct:source "ISO 31073:2022 Risk management vocabulary"@en ;
    rdfs:isDefinedBy risk-owl: ;
    rdfs:subClassOf rdfs:Class ;
    sw:term_status "accepted"@en ;
    skos:definition "Systematic application of management policies, procedures, and practices for communicating, consulting, establishing context, and identifying, analysing, evaluating, treating, monitoring and reviewing risk. ISO 31000 definition: coordinated activities to direct and control an organization with regard to risk"@en ;
    skos:prefLabel "Risk Management"@en .

risk-owl:RiskMatrix a rdfs:Class,
        owl:Class ;
    dct:contributor _:N0a43dd9ea5e94fe695d8b7df8802cfdd ;
    dct:created "2024-02-14"^^xsd:date ;
    dct:source [ a schema:WebPage ;
            schema:name "IEC 31010:2019" ;
            schema:url "https://www.iso.org/standard/72140.html" ] ;
    rdfs:isDefinedBy risk-owl: ;
    rdfs:subClassOf risk-owl:RiskAnalysis ;
    sw:term_status "accepted"@en ;
    skos:definition "Compares individual risks by selecting a consequence/ likelihood pair and displaying them on a matrix with consequence on one axis and likelihood on the other."@en ;
    skos:prefLabel "Risk Matrix"@en .

risk-owl:RiskOwner a rdfs:Class,
        owl:Class ;
    dct:created "2024-12-01"^^xsd:date ;
    rdfs:isDefinedBy risk-owl: ;
    rdfs:subClassOf risk-owl:RiskManagement ;
    sw:term_status "accepted"@en ;
    skos:definition "Entity accountable for managing risk"@en ;
    skos:prefLabel "Risk Owner"@en .

risk-owl:RiskPerception a rdfs:Class,
        owl:Class ;
    dct:created "2024-12-01"^^xsd:date ;
    rdfs:isDefinedBy risk-owl: ;
    rdfs:subClassOf risk-owl:RiskManagement ;
    sw:term_status "accepted"@en ;
    skos:definition "Perception or view on risk"@en ;
    skos:prefLabel "Risk Perception"@en .

risk-owl:RiskSource a rdfs:Class,
        owl:Class ;
    dct:created "2024-02-14"^^xsd:date ;
    dct:modified "2024-08-16"^^xsd:date ;
    rdfs:isDefinedBy risk-owl: ;
    rdfs:subClassOf risk-owl:RiskIdentification ;
    sw:term_status "accepted"@en ;
    skos:definition "The 'cause' or 'source', which by itself or with another source has the potential to give rise to risk"@en ;
    skos:prefLabel "Risk Source"@en .

risk-owl:RiskTreatment a rdfs:Class,
        owl:Class ;
    dct:created "2024-12-01"^^xsd:date ;
    rdfs:isDefinedBy risk-owl: ;
    rdfs:subClassOf risk-owl:RiskManagement ;
    sw:term_status "accepted"@en ;
    skos:definition "Process by which risk is modified and mitigated"@en ;
    skos:prefLabel "Risk Treatment"@en .

risk-owl:Threat a rdfs:Class,
        owl:Class ;
    dct:created "2024-02-14"^^xsd:date ;
    rdfs:isDefinedBy risk-owl: ;
    rdfs:subClassOf risk-owl:RiskIdentification ;
    sw:term_status "accepted"@en ;
    skos:definition "Risk source event which causes Risk"@en ;
    skos:prefLabel "Threat"@en .

risk-owl:ThreatSource a rdfs:Class,
        owl:Class ;
    dct:created "2024-02-14"^^xsd:date ;
    rdfs:isDefinedBy risk-owl: ;
    rdfs:subClassOf risk-owl:RiskIdentification ;
    sw:term_status "accepted"@en ;
    skos:definition "Source of threat event, including both agent and non-agent sources"@en ;
    skos:prefLabel "Threat Source"@en .

risk-owl:Vulnerability a rdfs:Class,
        owl:Class ;
    dct:created "2024-02-14"^^xsd:date ;
    rdfs:isDefinedBy risk-owl: ;
    rdfs:subClassOf risk-owl:RiskIdentification ;
    sw:term_status "accepted"@en ;
    skos:definition "Intrinsic property of a system or asset that is utilised by the Threat Source in a Threat event to cause Risk"@en ;
    skos:prefLabel "Vulnerability"@en .

risk-owl:causedByThreat a rdf:Property,
        owl:ObjectProperty ;
    dcam:rangeIncludes risk-owl:Threat ;
    dct:created "2024-02-14"^^xsd:date ;
    rdfs:isDefinedBy risk-owl: ;
    sw:term_status "accepted"@en ;
    skos:definition "Indicates the cause of associated context (subject) was the indicated threat (object)"@en ;
    skos:prefLabel "caused by threat"@en ;
    schema:rangeIncludes risk-owl:Threat .

risk-owl:causedByVulnerability a rdf:Property,
        owl:ObjectProperty ;
    dcam:rangeIncludes risk-owl:Vulnerability ;
    dct:created "2024-02-14"^^xsd:date ;
    rdfs:isDefinedBy risk-owl: ;
    sw:term_status "accepted"@en ;
    skos:definition "Indicates the associated context (subject) is caused by the indicated vulnerability (object)"@en ;
    skos:prefLabel "caused by vulnerability"@en ;
    schema:rangeIncludes risk-owl:Vulnerability .

risk-owl:exploitsVulnerability a rdf:Property,
        owl:ObjectProperty ;
    dcam:domainIncludes risk-owl:Threat ;
    dcam:rangeIncludes risk-owl:Vulnerability ;
    dct:created "2024-02-14"^^xsd:date ;
    rdfs:isDefinedBy risk-owl: ;
    sw:term_status "accepted"@en ;
    skos:definition "Indicates the threat (subject) exploits the indicated vulnerability (object)"@en ;
    skos:prefLabel "exploits vulnerability"@en ;
    schema:domainIncludes risk-owl:Threat ;
    schema:rangeIncludes risk-owl:Vulnerability .

risk-owl:hasRiskAcceptance a rdf:Property,
        owl:ObjectProperty ;
    dcam:rangeIncludes risk-owl:RiskAcceptance ;
    dct:created "2024-12-01"^^xsd:date ;
    rdfs:isDefinedBy risk-owl: ;
    sw:term_status "accepted"@en ;
    skos:definition "Associates the risk acceptance plan or process or criteria"@en ;
    skos:prefLabel "has risk acceptance"@en ;
    schema:rangeIncludes risk-owl:RiskAcceptance .

risk-owl:hasRiskAnalysis a rdf:Property,
        owl:ObjectProperty ;
    dcam:rangeIncludes risk-owl:RiskAnalysis ;
    dct:created "2024-12-01"^^xsd:date ;
    rdfs:isDefinedBy risk-owl: ;
    sw:term_status "accepted"@en ;
    skos:definition "Associates the risk analysis"@en ;
    skos:prefLabel "has risk analysis"@en ;
    schema:rangeIncludes risk-owl:RiskAnalysis .

risk-owl:hasRiskAssessment a rdf:Property,
        owl:ObjectProperty ;
    dcam:rangeIncludes risk-owl:RiskAssessment ;
    dct:created "2024-12-01"^^xsd:date ;
    rdfs:isDefinedBy risk-owl: ;
    sw:term_status "accepted"@en ;
    skos:definition "Associates the risk assessment"@en ;
    skos:prefLabel "has risk assessment"@en ;
    schema:rangeIncludes risk-owl:RiskAssessment .

risk-owl:hasRiskCriteria a rdf:Property,
        owl:ObjectProperty ;
    dcam:rangeIncludes risk-owl:RiskCriteria ;
    dct:created "2024-12-01"^^xsd:date ;
    rdfs:isDefinedBy risk-owl: ;
    sw:term_status "accepted"@en ;
    skos:definition "Associates the risk criteria"@en ;
    skos:prefLabel "has risk criteria"@en ;
    schema:rangeIncludes risk-owl:RiskCriteria .

risk-owl:hasRiskEvaluation a rdf:Property,
        owl:ObjectProperty ;
    dcam:rangeIncludes risk-owl:RiskEvaluation ;
    dct:created "2024-12-01"^^xsd:date ;
    rdfs:isDefinedBy risk-owl: ;
    sw:term_status "accepted"@en ;
    skos:definition "Associates the risk evaluation plan or process or criteria"@en ;
    skos:prefLabel "has risk evaluation"@en ;
    schema:rangeIncludes risk-owl:RiskEvaluation .

risk-owl:hasRiskIdentification a rdf:Property,
        owl:ObjectProperty ;
    dcam:rangeIncludes risk-owl:RiskIdentification ;
    dct:created "2024-12-01"^^xsd:date ;
    rdfs:isDefinedBy risk-owl: ;
    sw:term_status "accepted"@en ;
    skos:definition "Associates the risk identification plan or process or criteria"@en ;
    skos:prefLabel "has risk identification"@en ;
    schema:rangeIncludes risk-owl:RiskIdentification .

risk-owl:hasRiskManagement a rdf:Property,
        owl:ObjectProperty ;
    dcam:rangeIncludes risk-owl:RiskManagement ;
    dct:created "2024-12-01"^^xsd:date ;
    rdfs:isDefinedBy risk-owl: ;
    sw:term_status "accepted"@en ;
    skos:definition "Associates the risk management plan or process"@en ;
    skos:prefLabel "has risk management"@en ;
    schema:rangeIncludes risk-owl:RiskManagement .

risk-owl:hasRiskOwner a rdf:Property,
        owl:ObjectProperty ;
    dcam:rangeIncludes risk-owl:RiskOwner ;
    dct:created "2024-12-01"^^xsd:date ;
    rdfs:isDefinedBy risk-owl: ;
    sw:term_status "accepted"@en ;
    skos:definition "Indicates the risk owner"@en ;
    skos:prefLabel "has risk owner"@en ;
    schema:rangeIncludes risk-owl:RiskOwner .

risk-owl:hasRiskPerception a rdf:Property,
        owl:ObjectProperty ;
    dcam:rangeIncludes risk-owl:RiskPerception ;
    dct:created "2024-12-01"^^xsd:date ;
    rdfs:isDefinedBy risk-owl: ;
    sw:term_status "accepted"@en ;
    skos:definition "Associates the risk perception plan or process or criteria"@en ;
    skos:prefLabel "has risk perception"@en ;
    schema:rangeIncludes risk-owl:RiskPerception .

risk-owl:hasRiskSource a rdf:Property,
        owl:ObjectProperty ;
    dcam:domainIncludes dpv-owl:Risk ;
    dcam:rangeIncludes risk-owl:RiskSource ;
    dct:created "2024-02-14"^^xsd:date ;
    rdfs:isDefinedBy risk-owl: ;
    sw:term_status "accepted"@en ;
    skos:definition "Indicates the risk (subject) has the indicated risk source (object)"@en ;
    skos:prefLabel "has risk source"@en ;
    schema:domainIncludes dpv-owl:Risk ;
    schema:rangeIncludes risk-owl:RiskSource .

risk-owl:hasRiskTreatment a rdf:Property,
        owl:ObjectProperty ;
    dcam:rangeIncludes risk-owl:RiskTreatment ;
    dct:created "2024-12-01"^^xsd:date ;
    rdfs:isDefinedBy risk-owl: ;
    sw:term_status "accepted"@en ;
    skos:definition "Associates the risk treatment plan or process or criteria"@en ;
    skos:prefLabel "has risk treatment"@en ;
    schema:rangeIncludes risk-owl:RiskTreatment .

risk-owl:hasThreatSource a rdf:Property,
        owl:ObjectProperty ;
    dcam:domainIncludes risk-owl:Threat ;
    dcam:rangeIncludes risk-owl:ThreatSource ;
    dct:created "2024-02-14"^^xsd:date ;
    rdfs:isDefinedBy risk-owl: ;
    sw:term_status "accepted"@en ;
    skos:definition "Indicates the threat (subject) has the indicated source (object)"@en ;
    skos:prefLabel "has threat source"@en ;
    schema:domainIncludes risk-owl:Threat ;
    schema:rangeIncludes risk-owl:ThreatSource .

risk-owl:hasVulnerability a rdf:Property,
        owl:ObjectProperty ;
    dcam:rangeIncludes risk-owl:Vulnerability ;
    dct:created "2024-02-14"^^xsd:date ;
    rdfs:isDefinedBy risk-owl: ;
    sw:term_status "accepted"@en ;
    skos:definition "Indicates the associated context (subject) has indicated vulnerability (object)"@en ;
    skos:prefLabel "has vulnerability"@en ;
    schema:rangeIncludes risk-owl:Vulnerability .

risk-owl:isExploitedBy a rdf:Property,
        owl:ObjectProperty ;
    dcam:domainIncludes risk-owl:Vulnerability ;
    dcam:rangeIncludes risk-owl:Threat ;
    dct:created "2024-02-14"^^xsd:date ;
    rdfs:isDefinedBy risk-owl: ;
    sw:term_status "accepted"@en ;
    skos:definition "Indicates the vulnerability (subject) is exploited by the indicated threat (object)"@en ;
    skos:prefLabel "is exploited by"@en ;
    schema:domainIncludes risk-owl:Vulnerability ;
    schema:rangeIncludes risk-owl:Threat .

risk-owl:isVulnerabilityOf a rdf:Property,
        owl:ObjectProperty ;
    dcam:domainIncludes risk-owl:Vulnerability ;
    dct:created "2024-02-14"^^xsd:date ;
    rdfs:isDefinedBy risk-owl: ;
    sw:term_status "accepted"@en ;
    skos:definition "Indicates the vulnerability (subject) is associated with indicated context (object)"@en ;
    skos:prefLabel "is vulnerability of"@en ;
    schema:domainIncludes risk-owl:Vulnerability .

risk-owl:refersToRisk a rdf:Property,
        owl:ObjectProperty ;
    dcam:domainIncludes dpv-owl:Incident ;
    dcam:rangeIncludes dpv-owl:Risk ;
    dct:created "2024-02-14"^^xsd:date ;
    vann:example dex-owl:E0069 ;
    rdfs:isDefinedBy risk-owl: ;
    sw:term_status "accepted"@en ;
    skos:definition "Indicates the incident (subject) is a materialisation of the indicated risk (object)"@en ;
    skos:prefLabel "refers to risk"@en ;
    schema:domainIncludes dpv-owl:Incident ;
    schema:rangeIncludes dpv-owl:Risk .

risk-owl:serialisation-html a profile:ResourceDescriptor ;
    dct:conformsTo <https://www.w3.org/TR/html/> ;
    dct:format <https://www.iana.org/assignments/media-types/text/html> ;
    dct:title "Risk Concepts - HTML serialiation" ;
    profile:hasArtifact <https://w3id.org/dpv/risk/risk-owl.html> ;
    profile:hasRole role:specification .

risk-owl:serialisation-jsonld a profile:ResourceDescriptor ;
    dct:conformsTo <https://www.w3.org/TR/json-ld11/> ;
    dct:format <https://www.iana.org/assignments/media-types/application/ld+json> ;
    dct:title "Risk Concepts - JSON-LD serialiation" ;
    profile:hasArtifact <https://w3id.org/dpv/risk/risk-owl.jsonld> ;
    profile:hasRole role:vocabulary .

risk-owl:serialisation-n3 a profile:ResourceDescriptor ;
    dct:conformsTo <https://www.w3.org/TeamSubmission/n3/> ;
    dct:format <https://www.iana.org/assignments/media-types/text/n3> ;
    dct:title "Risk Concepts - N3 serialiation" ;
    profile:hasArtifact <https://w3id.org/dpv/risk/risk-owl.n3> ;
    profile:hasRole role:vocabulary .

risk-owl:serialisation-rdf a profile:ResourceDescriptor ;
    dct:conformsTo rdf: ;
    dct:format <https://www.iana.org/assignments/media-types/application/rdf+xml> ;
    dct:title "Risk Concepts - RDF/XML serialiation" ;
    profile:hasArtifact <https://w3id.org/dpv/risk/risk-owl.rdf> ;
    profile:hasRole role:vocabulary .

risk-owl:serialisation-ttl a profile:ResourceDescriptor ;
    dct:conformsTo <https://www.w3.org/TR/turtle/> ;
    dct:format <https://www.iana.org/assignments/media-types/text/turtle> ;
    dct:title "Risk Concepts - Turtle serialiation" ;
    profile:hasArtifact <https://w3id.org/dpv/risk/risk-owl.ttl> ;
    profile:hasRole role:vocabulary .

<https://w3id.org/dpv/examples> a profile:ResourceDescriptor ;
    dct:conformsTo <https://www.w3.org/TR/html/> ;
    dct:format <https://www.iana.org/assignments/media-types/text/html> ;
    dct:title "Examples for Data Privacy Vocabulary" ;
    profile:hasArtifact <https://w3id.org/dpv/examples> ;
    profile:hasRole role:guidance .

<https://w3id.org/dpv/guides> a profile:ResourceDescriptor ;
    dct:conformsTo <https://www.w3.org/TR/html/> ;
    dct:format <https://www.iana.org/assignments/media-types/text/html> ;
    dct:title "Guides for Data Privacy Vocabulary" ;
    profile:hasArtifact <https://w3id.org/dpv/guides> ;
    profile:hasRole role:guidance .

<https://w3id.org/dpv/primer> a profile:ResourceDescriptor ;
    dct:conformsTo <https://www.w3.org/TR/html/> ;
    dct:format <https://www.iana.org/assignments/media-types/text/html> ;
    dct:title "Primer for Data Privacy Vocabulary" ;
    profile:hasArtifact <https://w3id.org/dpv/primer> ;
    profile:hasRole role:guidance .

risk-owl: a owl:Ontology,
        profile:Profile ;
    dct:bibliographicCitation "Harshvardhan J. Pandit, Beatriz Esteves, Georg P. Krog, Paul Ryan, Delaram Golpayegani, Julian Flake (2025) Data Privacy Vocabulary (DPV) – Version 2.0. In: Demartini, G., et al. The Semantic Web – ISWC 2024. ISWC 2024. Lecture Notes in Computer Science, vol 15233. Springer, Cham. https://doi.org/10.1007/978-3-031-77847-6_10" ;
    dct:conformsTo <http://www.w3.org/2002/07/owl>,
        "http://www.w3.org/2000/01/rdf-schema",
        "http://www.w3.org/2004/02/skos/core" ;
    dct:contributor _:N0a43dd9ea5e94fe695d8b7df8802cfdd ;
    dct:created "2022-08-14"@en ;
    dct:creator [ a dct:Agent,
                foaf:Person ;
            org:memberOf [ a foaf:Organization ;
                    foaf:name "Signatu AS" ] ;
            foaf:homepage "https://www.linkedin.com/in/georg-philip-krog-a2a278104/" ;
            foaf:name "Georg P. Krog" ],
        _:N0a43dd9ea5e94fe695d8b7df8802cfdd,
        [ a dct:Agent,
                foaf:Person ;
            scoro:hasORCID "0009-0006-4623-1463" ;
            org:memberOf [ a foaf:Organization ;
                    foaf:name "University of Koblenz" ] ;
            foaf:name "Julian Flake" ],
        [ a dct:Agent,
                foaf:Person ;
            org:memberOf [ a foaf:Organization ;
                    foaf:name "University College Dublin" ] ;
            foaf:name "Rob Brennan" ],
        [ a dct:Agent,
                foaf:Person ;
            scoro:hasORCID "0000-0003-0259-7560" ;
            org:memberOf [ a foaf:Organization ;
                    foaf:name "IDLab, IMEC, Ghent University" ] ;
            foaf:name "Beatriz Esteves" ],
        [ a dct:Agent,
                foaf:Person ;
            scoro:hasORCID "0000-0003-0770-2737" ;
            org:memberOf [ a foaf:Organization ;
                    foaf:name "Uniphar PLC" ] ;
            foaf:name "Paul Ryan" ],
        [ a dct:Agent,
                foaf:Person ;
            scoro:hasORCID "0000-0002-1208-186X" ;
            org:memberOf [ a foaf:Organization ;
                    foaf:name "ADAPT Centre, Trinity College Dublin" ] ;
            foaf:name "Delaram Golpayegani" ] ;
    dct:description "Extension to the Data Privacy Vocabulary (DPV) providing concepts for representing information about risk assessment and risk management"@en ;
    dct:hasVersion risk-owl: ;
    dct:identifier "https://w3id.org/dpv/risk" ;
    dct:issued "2022-08-14"@en ;
    dct:license <https://www.w3.org/copyright/document-license-2023/> ;
    dct:modified "2025-03-16"@en ;
    dct:publisher <https://www.w3.org/> ;
    dct:source <https://www.w3.org/groups/cg/dpvcg/> ;
    dct:title "Risk Concepts"@en ;
    bibo:doi "10.5281/zenodo.12505841" ;
    bibo:status "http://purl.org/ontology/bibo/status/published" ;
    vann:preferredNamespacePrefix "risk" ;
    vann:preferredNamespaceUri "https://w3id.org/dpv/risk#" ;
    rdfs:Label "RISK"@en ;
    owl:versionIRI <https://w3id.org/dpv/2.1/risk/owl#> ;
    owl:versionInfo "2.1" ;
    profile:hasResource <https://w3id.org/dpv/examples>,
        <https://w3id.org/dpv/guides>,
        <https://w3id.org/dpv/primer>,
        risk-owl:serialisation-html,
        risk-owl:serialisation-jsonld,
        risk-owl:serialisation-n3,
        risk-owl:serialisation-rdf,
        risk-owl:serialisation-ttl ;
    profile:isProfileOf <http://www.w3.org/2002/07/owl>,
        <https://w3id.org/dpv/owl>,
        risk-owl: ;
    foaf:logo <https://w3id.org/dpv/media/logo.png> ;
    schema:version "2.1" .

_:N313d89a6c37147bfac1bbb4aa7f6510b a foaf:Organization ;
    foaf:name "ADAPT Centre, Dublin City University" .

_:N0a43dd9ea5e94fe695d8b7df8802cfdd a dct:Agent,
        foaf:Person ;
    scoro:hasORCID "0000-0002-5068-3714" ;
    org:memberOf _:N313d89a6c37147bfac1bbb4aa7f6510b ;
    foaf:homepage "https://harshp.com/" ;
    foaf:name "Harshvardhan J. Pandit" .

