@prefix bibo: <http://purl.org/ontology/bibo/> .
@prefix dct: <http://purl.org/dc/terms/> .
@prefix dpv-owl: <https://w3id.org/dpv/owl#> .
@prefix foaf: <http://xmlns.com/foaf/0.1/> .
@prefix org: <http://www.w3.org/ns/org#> .
@prefix owl: <http://www.w3.org/2002/07/owl#> .
@prefix profile: <http://www.w3.org/ns/dx/prof/> .
@prefix rdf: <http://www.w3.org/1999/02/22-rdf-syntax-ns#> .
@prefix rdfs: <http://www.w3.org/2000/01/rdf-schema#> .
@prefix role: <http://www.w3.org/ns/dx/prof/role/> .
@prefix schema: <https://schema.org/> .
@prefix scoro: <http://purl.org/spar/scoro/> .
@prefix sector-infra-owl: <https://w3id.org/dpv/sector/infra/owl#> .
@prefix skos: <http://www.w3.org/2004/02/skos/core#> .
@prefix sw: <http://www.w3.org/2003/06/sw-vocab-status/ns#> .
@prefix vann: <http://purl.org/vocab/vann/> .
@prefix xsd: <http://www.w3.org/2001/XMLSchema#> .

sector-infra-owl:AviationInfrastructureManagement a rdfs:Class,
        owl:Class,
        dpv-owl:Purpose ;
    dct:created "2024-12-01"^^xsd:date ;
    rdfs:isDefinedBy sector-infra-owl: ;
    rdfs:subClassOf sector-infra-owl:TransportManagement ;
    sw:term_status "accepted"@en ;
    skos:definition "Purposes associated with management of aviation transport infrastructure"@en ;
    skos:prefLabel "Aviation Infrastructure Management"@en .

sector-infra-owl:CriticalCommunicationManagement a rdfs:Class,
        owl:Class,
        dpv-owl:Purpose ;
    dct:created "2024-12-01"^^xsd:date ;
    rdfs:isDefinedBy sector-infra-owl: ;
    rdfs:subClassOf sector-infra-owl:CriticalInfrastructureManagement ;
    sw:term_status "accepted"@en ;
    skos:definition "Purposes associated with management of critical communications infrastructure and services"@en ;
    skos:prefLabel "Critical Communication Management"@en .

sector-infra-owl:CriticalDigitalInfrastructureManagement a rdfs:Class,
        owl:Class,
        dpv-owl:Purpose ;
    dct:created "2024-12-01"^^xsd:date ;
    rdfs:isDefinedBy sector-infra-owl: ;
    rdfs:subClassOf sector-infra-owl:CriticalInfrastructureManagement ;
    sw:term_status "accepted"@en ;
    skos:definition "Purposes associated with management of digital infrastructure considered as part of critical infrastructure"@en ;
    skos:prefLabel "Critical Digital Infrastructure Management"@en .

sector-infra-owl:CriticalElectricityManagement a rdfs:Class,
        owl:Class,
        dpv-owl:Purpose ;
    dct:created "2024-12-01"^^xsd:date ;
    rdfs:isDefinedBy sector-infra-owl: ;
    rdfs:subClassOf sector-infra-owl:CriticalEnergyManagement ;
    sw:term_status "accepted"@en ;
    skos:definition "Purposes associated with management of critical electric energy infrastructure and services"@en ;
    skos:prefLabel "Critical Electricity Management"@en .

sector-infra-owl:CriticalEmergencyResponseCommunicationManagement a rdfs:Class,
        owl:Class,
        dpv-owl:Purpose ;
    dct:created "2024-12-01"^^xsd:date ;
    rdfs:isDefinedBy sector-infra-owl: ;
    rdfs:subClassOf sector-infra-owl:CriticalEmergencyResponseManagement ;
    sw:term_status "accepted"@en ;
    skos:definition "Purposes associated with communications involved to request and use emergency response services such as fire fighters and paramedics considered as part of critical infrastructure"@en ;
    skos:prefLabel "Critical Emergency Response Communication Management"@en .

sector-infra-owl:CriticalEmergencyResponseDispatchManagement a rdfs:Class,
        owl:Class,
        dpv-owl:Purpose ;
    dct:created "2024-12-01"^^xsd:date ;
    rdfs:isDefinedBy sector-infra-owl: ;
    rdfs:subClassOf sector-infra-owl:CriticalEmergencyResponseManagement ;
    sw:term_status "accepted"@en ;
    skos:definition "Purposes associated with identifying routes and other dispatch related activities for emergency response services such as fire fighters and paramedics considered as part of critical infrastructure"@en ;
    skos:prefLabel "Critical Emergency Response Dispatch Management"@en .

sector-infra-owl:CriticalEmergencyResponseEligibilityAssessment a rdfs:Class,
        owl:Class,
        dpv-owl:Purpose ;
    dct:created "2024-12-01"^^xsd:date ;
    rdfs:isDefinedBy sector-infra-owl: ;
    rdfs:subClassOf sector-infra-owl:CriticalEmergencyResponseManagement ;
    sw:term_status "accepted"@en ;
    skos:definition "Purposes associated with assessment of eligibility to dispatch and use emergency response services such as fire fighters and paramedics considered as part of critical infrastructure"@en ;
    skos:prefLabel "Critical Emergency Response Eligibility Assessment"@en .

sector-infra-owl:CriticalEmergencyResponseManagement a rdfs:Class,
        owl:Class,
        dpv-owl:Purpose ;
    dct:created "2024-12-01"^^xsd:date ;
    rdfs:isDefinedBy sector-infra-owl: ;
    rdfs:subClassOf sector-infra-owl:CriticalInfrastructureManagement ;
    sw:term_status "accepted"@en ;
    skos:definition "Purposes associated with management of emergency response services such as fire fighters and paramedics considered as part of critical infrastructure"@en ;
    skos:prefLabel "Critical Emergency Response Management"@en .

sector-infra-owl:CriticalEmergencyResponseTriage a rdfs:Class,
        owl:Class,
        dpv-owl:Purpose ;
    dct:created "2024-12-01"^^xsd:date ;
    rdfs:isDefinedBy sector-infra-owl: ;
    rdfs:subClassOf sector-infra-owl:CriticalEmergencyResponseManagement ;
    sw:term_status "accepted"@en ;
    skos:definition "Purposes associated with prioritisation and other triage procedures to dispatch and use emergency response services such as fire fighters and paramedics considered as part of critical infrastructure"@en ;
    skos:prefLabel "Critical Emergency Response Triage"@en .

sector-infra-owl:CriticalEnergyManagement a rdfs:Class,
        owl:Class,
        dpv-owl:Purpose ;
    dct:created "2024-12-01"^^xsd:date ;
    rdfs:isDefinedBy sector-infra-owl: ;
    rdfs:subClassOf sector-infra-owl:CriticalInfrastructureManagement ;
    sw:term_status "accepted"@en ;
    skos:definition "Purposes associated with management of critical energy infrastructure and services"@en ;
    skos:prefLabel "Critical Energy Management"@en .

sector-infra-owl:CriticalGasManagement a rdfs:Class,
        owl:Class,
        dpv-owl:Purpose ;
    dct:created "2024-12-01"^^xsd:date ;
    rdfs:isDefinedBy sector-infra-owl: ;
    rdfs:subClassOf sector-infra-owl:CriticalEnergyManagement ;
    sw:term_status "accepted"@en ;
    skos:definition "Purposes associated with management of critical gas energy infrastructure and services"@en ;
    skos:prefLabel "Critical Gas Management"@en .

sector-infra-owl:CriticalHeatingManagement a rdfs:Class,
        owl:Class,
        dpv-owl:Purpose ;
    dct:created "2024-12-01"^^xsd:date ;
    rdfs:isDefinedBy sector-infra-owl: ;
    rdfs:subClassOf sector-infra-owl:CriticalInfrastructureManagement ;
    sw:term_status "accepted"@en ;
    skos:definition "Purposes associated with management of critical heating infrastructure and services"@en ;
    skos:prefLabel "Critical Heating Management"@en .

sector-infra-owl:CriticalInfrastructureManagement a rdfs:Class,
        owl:Class,
        dpv-owl:Purpose ;
    dct:created "2024-12-01"^^xsd:date ;
    rdfs:isDefinedBy sector-infra-owl: ;
    rdfs:subClassOf sector-infra-owl:InfrastructureManagement ;
    sw:term_status "accepted"@en ;
    skos:definition "Purposes associated with management of infrastructure considered essential or critical for functioning of society and economy as defined by a government or a legislation"@en ;
    skos:prefLabel "Critical Infrastructure Management"@en .

sector-infra-owl:CriticalWasteManagement a rdfs:Class,
        owl:Class,
        dpv-owl:Purpose ;
    dct:created "2024-12-01"^^xsd:date ;
    rdfs:isDefinedBy sector-infra-owl: ;
    rdfs:subClassOf sector-infra-owl:CriticalInfrastructureManagement ;
    sw:term_status "accepted"@en ;
    skos:definition "Purposes associated with management of waste collection and management considered as part of critical infrastructure"@en ;
    skos:prefLabel "Critical Waste Management"@en .

sector-infra-owl:CriticalWaterManagement a rdfs:Class,
        owl:Class,
        dpv-owl:Purpose ;
    dct:created "2024-12-01"^^xsd:date ;
    rdfs:isDefinedBy sector-infra-owl: ;
    rdfs:subClassOf sector-infra-owl:CriticalInfrastructureManagement ;
    sw:term_status "accepted"@en ;
    skos:definition "Purposes associated with management of critical water infrastructure and services"@en ;
    skos:prefLabel "Critical Water Management"@en .

sector-infra-owl:InfrastructureManagement a rdfs:Class,
        owl:Class,
        dpv-owl:Purpose ;
    dct:created "2024-12-01"^^xsd:date ;
    rdfs:isDefinedBy sector-infra-owl: ;
    rdfs:subClassOf dpv-owl:Purpose ;
    sw:term_status "accepted"@en ;
    skos:definition "Purposes associated with management of infrastructure"@en ;
    skos:prefLabel "Infrastructure Management"@en .

sector-infra-owl:PublicTransportComplaintManagement a rdfs:Class,
        owl:Class,
        dpv-owl:Purpose ;
    dct:created "2024-12-01"^^xsd:date ;
    rdfs:isDefinedBy sector-infra-owl: ;
    rdfs:subClassOf sector-infra-owl:PublicTransportManagement ;
    sw:term_status "accepted"@en ;
    skos:definition "Purposes associated with collection, resolution, and analysis of complaints in relation to use of public transport services"@en ;
    skos:prefLabel "Public Transport Complaint Management"@en .

sector-infra-owl:PublicTransportDemandForecasting a rdfs:Class,
        owl:Class,
        dpv-owl:Purpose ;
    dct:created "2024-12-01"^^xsd:date ;
    rdfs:isDefinedBy sector-infra-owl: ;
    rdfs:subClassOf sector-infra-owl:PublicTransportResearchDevelopment ;
    sw:term_status "accepted"@en ;
    skos:definition "Purposes associated with predicting demand in relation to public transport services"@en ;
    skos:prefLabel "Public Transport Demand Forecasting"@en .

sector-infra-owl:PublicTransportFraudManagement a rdfs:Class,
        owl:Class,
        dpv-owl:Purpose ;
    dct:created "2024-12-01"^^xsd:date ;
    rdfs:isDefinedBy sector-infra-owl: ;
    rdfs:subClassOf dpv-owl:PublicBenefit,
        sector-infra-owl:PublicTransportManagement ;
    sw:term_status "accepted"@en ;
    skos:definition "Purposes associated with detection, resolution, and analysis of fraud in use of public transport services"@en ;
    skos:prefLabel "Public Transport Fraud Management"@en .

sector-infra-owl:PublicTransportManagement a rdfs:Class,
        owl:Class,
        dpv-owl:Purpose ;
    dct:created "2024-12-01"^^xsd:date ;
    rdfs:isDefinedBy sector-infra-owl: ;
    rdfs:subClassOf dpv-owl:PublicBenefit,
        sector-infra-owl:TransportManagement ;
    sw:term_status "accepted"@en ;
    skos:definition "Purposes associated with management of public transport services"@en ;
    skos:prefLabel "Public Transport Management"@en .

sector-infra-owl:PublicTransportPassengerFlowAnalysis a rdfs:Class,
        owl:Class,
        dpv-owl:Purpose ;
    dct:created "2024-12-01"^^xsd:date ;
    rdfs:isDefinedBy sector-infra-owl: ;
    rdfs:subClassOf sector-infra-owl:PublicTransportResearchDevelopment ;
    sw:term_status "accepted"@en ;
    skos:definition "Purposes associated with analysis of passenger movements in relation to use of public transport services, such as for identifying which areas are most busy on specific days"@en ;
    skos:prefLabel "Public Transport Passenger Flow Analysis"@en .

sector-infra-owl:PublicTransportPerformanceAnalysis a rdfs:Class,
        owl:Class,
        dpv-owl:Purpose ;
    dct:created "2024-12-01"^^xsd:date ;
    rdfs:isDefinedBy sector-infra-owl: ;
    rdfs:subClassOf sector-infra-owl:PublicTransportResearchDevelopment ;
    sw:term_status "accepted"@en ;
    skos:definition "Purposes associated with analysis of performance and other characteristics  with the goal of identifying and making improvements related to public transport services"@en ;
    skos:prefLabel "Public Transport Performance Analysis"@en .

sector-infra-owl:PublicTransportResearchDevelopment a rdfs:Class,
        owl:Class,
        dpv-owl:Purpose ;
    dct:created "2024-12-01"^^xsd:date ;
    rdfs:isDefinedBy sector-infra-owl: ;
    rdfs:subClassOf dpv-owl:PublicBenefit,
        dpv-owl:ResearchAndDevelopment,
        sector-infra-owl:PublicTransportManagement ;
    sw:term_status "accepted"@en ;
    skos:definition "Purposes associated with research and development activities in relation to public transport services"@en ;
    skos:prefLabel "Public Transport Research Development"@en .

sector-infra-owl:PublicTransportSafetyManagement a rdfs:Class,
        owl:Class,
        dpv-owl:Purpose ;
    dct:created "2024-12-01"^^xsd:date ;
    rdfs:isDefinedBy sector-infra-owl: ;
    rdfs:subClassOf dpv-owl:PublicBenefit,
        sector-infra-owl:PublicTransportManagement ;
    sw:term_status "accepted"@en ;
    skos:definition "Purposes associated with management of safety in use of public transport services, such as through deployment of CCTV cameras in buses or on public transport premises"@en ;
    skos:prefLabel "Public Transport Safety Management"@en .

sector-infra-owl:PublicTransportServiceProvision a rdfs:Class,
        owl:Class,
        dpv-owl:Purpose ;
    dct:created "2024-12-01"^^xsd:date ;
    rdfs:isDefinedBy sector-infra-owl: ;
    rdfs:subClassOf sector-infra-owl:PublicTransportManagement ;
    sw:term_status "accepted"@en ;
    skos:definition "Purposes associated with provision of public transport services"@en ;
    skos:prefLabel "Public Transport Service Provision"@en .

sector-infra-owl:PublicTransportTicketManagement a rdfs:Class,
        owl:Class,
        dpv-owl:Purpose ;
    dct:created "2024-12-01"^^xsd:date ;
    rdfs:isDefinedBy sector-infra-owl: ;
    rdfs:subClassOf sector-infra-owl:PublicTransportServiceProvision ;
    sw:term_status "accepted"@en ;
    skos:definition "Purposes associated with management of ticketing and other forms of documentation enabling use of public transport services"@en ;
    skos:prefLabel "Public Transport Ticket Management"@en .

sector-infra-owl:RailTransportManagement a rdfs:Class,
        owl:Class,
        dpv-owl:Purpose ;
    dct:created "2024-12-01"^^xsd:date ;
    rdfs:isDefinedBy sector-infra-owl: ;
    rdfs:subClassOf sector-infra-owl:TransportManagement ;
    sw:term_status "accepted"@en ;
    skos:definition "Purposes associated with management of rail transport infrastructure"@en ;
    skos:prefLabel "Rail Transport Management"@en .

sector-infra-owl:RoadAccidentAnalysis a rdfs:Class,
        owl:Class,
        dpv-owl:Purpose ;
    dct:created "2024-12-01"^^xsd:date ;
    rdfs:isDefinedBy sector-infra-owl: ;
    rdfs:subClassOf sector-infra-owl:RoadResearchDevelopment ;
    sw:term_status "accepted"@en ;
    skos:definition "Purposes associated with analysis of accidens with the goal of researching and developing improvements to road infrastructure"@en ;
    skos:prefLabel "Road Accident Analysis"@en .

sector-infra-owl:RoadAccidentMonitoring a rdfs:Class,
        owl:Class,
        dpv-owl:Purpose ;
    dct:created "2024-12-01"^^xsd:date ;
    rdfs:isDefinedBy sector-infra-owl: ;
    rdfs:subClassOf sector-infra-owl:RoadSafetyMonitoring ;
    sw:term_status "accepted"@en ;
    skos:definition "Purposes associated with monitoring of accidents on roads"@en ;
    skos:prefLabel "Road Accident Monitoring"@en .

sector-infra-owl:RoadConditionMonitoring a rdfs:Class,
        owl:Class,
        dpv-owl:Purpose ;
    dct:created "2024-12-01"^^xsd:date ;
    rdfs:isDefinedBy sector-infra-owl: ;
    rdfs:subClassOf sector-infra-owl:RoadSafetyMonitoring ;
    sw:term_status "accepted"@en ;
    skos:definition "Purposes associated with monitoring of road conditions, including weather conditions for safety"@en ;
    skos:prefLabel "Road Condition Monitoring"@en .

sector-infra-owl:RoadEmergencyResponseManagement a rdfs:Class,
        owl:Class,
        dpv-owl:Purpose ;
    dct:created "2024-12-01"^^xsd:date ;
    rdfs:isDefinedBy sector-infra-owl: ;
    rdfs:subClassOf sector-infra-owl:RoadManagement ;
    sw:term_status "accepted"@en ;
    skos:definition "Purposes associated with management of emergency response and other safety activities in relation to emergencies in use of road transport infrastructure"@en ;
    skos:prefLabel "Road Emergency Response Management"@en .

sector-infra-owl:RoadEmergencyRouteManagement a rdfs:Class,
        owl:Class,
        dpv-owl:Purpose ;
    dct:created "2024-12-01"^^xsd:date ;
    rdfs:isDefinedBy sector-infra-owl: ;
    rdfs:subClassOf sector-infra-owl:RoadEmergencyResponseManagement ;
    sw:term_status "accepted"@en ;
    skos:definition "Purposes associated with management of routes used for emergency response or managing traffic in response to an emergency response in use of road transport infrastructure"@en ;
    skos:prefLabel "Road Emergency Route Management"@en .

sector-infra-owl:RoadEmergencySceneManagement a rdfs:Class,
        owl:Class,
        dpv-owl:Purpose ;
    dct:created "2024-12-01"^^xsd:date ;
    rdfs:isDefinedBy sector-infra-owl: ;
    rdfs:subClassOf sector-infra-owl:RoadEmergencyResponseManagement ;
    sw:term_status "accepted"@en ;
    skos:definition "Purposes associated with management of the scene during an accident or other emergencies in use of road transport infrastructure"@en ;
    skos:prefLabel "Road Emergency Scene Management"@en .

sector-infra-owl:RoadEnvironmentalImpactAnalysis a rdfs:Class,
        owl:Class,
        dpv-owl:Purpose ;
    dct:created "2024-12-01"^^xsd:date ;
    rdfs:isDefinedBy sector-infra-owl: ;
    rdfs:subClassOf sector-infra-owl:RoadResearchDevelopment ;
    sw:term_status "accepted"@en ;
    skos:definition "Purposes associated with conducting environmental impact analysis regarding use and development of road infrastructure"@en ;
    skos:prefLabel "Road Environmental Impact Analysis"@en .

sector-infra-owl:RoadInfrastructureManagement a rdfs:Class,
        owl:Class,
        dpv-owl:Purpose ;
    dct:created "2024-12-01"^^xsd:date ;
    rdfs:isDefinedBy sector-infra-owl: ;
    rdfs:subClassOf sector-infra-owl:TransportManagement ;
    sw:term_status "accepted"@en ;
    skos:definition "Purposes associated with management of road transport infrastructure"@en ;
    skos:prefLabel "Road Infrastructure Management"@en .

sector-infra-owl:RoadInfrastructurePlanning a rdfs:Class,
        owl:Class,
        dpv-owl:Purpose ;
    dct:created "2024-12-01"^^xsd:date ;
    rdfs:isDefinedBy sector-infra-owl: ;
    rdfs:subClassOf dpv-owl:PublicBenefit,
        dpv-owl:ResearchAndDevelopment,
        sector-infra-owl:RoadResearchDevelopment ;
    sw:term_status "accepted"@en ;
    skos:definition "Purposes associated with planning road infrastructure"@en ;
    skos:prefLabel "Road Infrastructure Planning"@en .

sector-infra-owl:RoadMaintenanceScheduling a rdfs:Class,
        owl:Class,
        dpv-owl:Purpose ;
    dct:created "2024-12-01"^^xsd:date ;
    rdfs:isDefinedBy sector-infra-owl: ;
    rdfs:subClassOf sector-infra-owl:RoadManagement ;
    sw:term_status "accepted"@en ;
    skos:definition "Purposes associated with scheduling and managing road maintainence"@en ;
    skos:prefLabel "Road Maintenance Scheduling"@en .

sector-infra-owl:RoadManagement a rdfs:Class,
        owl:Class,
        dpv-owl:Purpose ;
    dct:created "2024-12-01"^^xsd:date ;
    rdfs:isDefinedBy sector-infra-owl: ;
    rdfs:subClassOf sector-infra-owl:RoadInfrastructureManagement ;
    sw:term_status "accepted"@en ;
    skos:definition "Purposes associated with management of roads as a transport infrastructure"@en ;
    skos:prefLabel "Road Management"@en .

sector-infra-owl:RoadPedestrianSafetyMonitoring a rdfs:Class,
        owl:Class,
        dpv-owl:Purpose ;
    dct:created "2024-12-01"^^xsd:date ;
    rdfs:isDefinedBy sector-infra-owl: ;
    rdfs:subClassOf sector-infra-owl:RoadSafetyMonitoring ;
    sw:term_status "accepted"@en ;
    skos:definition "Purposes associated with monitoring of conditions, pedestrians, and traffic for safety related to use of roads for pedestrians"@en ;
    skos:prefLabel "Road Pedestrian Safety Monitoring"@en .

sector-infra-owl:RoadResearchDevelopment a rdfs:Class,
        owl:Class,
        dpv-owl:Purpose ;
    dct:created "2024-12-01"^^xsd:date ;
    rdfs:isDefinedBy sector-infra-owl: ;
    rdfs:subClassOf sector-infra-owl:RoadManagement ;
    sw:term_status "accepted"@en ;
    skos:definition "Purposes associated with management of research and development for road infrastructure, including planning changes and new infrastructure, analysing traffic and accident patterns, and environmental impact analysis"@en ;
    skos:prefLabel "Road Research Development"@en .

sector-infra-owl:RoadSafetyMonitoring a rdfs:Class,
        owl:Class,
        dpv-owl:Purpose ;
    dct:created "2024-12-01"^^xsd:date ;
    rdfs:isDefinedBy sector-infra-owl: ;
    rdfs:subClassOf sector-infra-owl:RoadManagement ;
    sw:term_status "accepted"@en ;
    skos:definition "Purposes associated with management of road safety"@en ;
    skos:prefLabel "Road Safety Monitoring"@en .

sector-infra-owl:RoadSchoolZoneSafetyMonitoring a rdfs:Class,
        owl:Class,
        dpv-owl:Purpose ;
    dct:created "2024-12-01"^^xsd:date ;
    rdfs:isDefinedBy sector-infra-owl: ;
    rdfs:subClassOf sector-infra-owl:RoadSafetyMonitoring ;
    sw:term_status "accepted"@en ;
    skos:definition "Purposes associated with monitoring of conditions, pedestrians, and traffic for safety in an area nearby or including a school or other similar institutes"@en ;
    skos:prefLabel "Road School Zone Safety Monitoring"@en .

sector-infra-owl:RoadTollCollection a rdfs:Class,
        owl:Class,
        dpv-owl:Purpose ;
    dct:created "2024-12-01"^^xsd:date ;
    rdfs:isDefinedBy sector-infra-owl: ;
    rdfs:subClassOf sector-infra-owl:RoadTollManagement ;
    sw:term_status "accepted"@en ;
    skos:definition "Purposes associated with collection of tolls and other forms of fees for use of road transport infrastructure"@en ;
    skos:prefLabel "Road Toll Collection"@en .

sector-infra-owl:RoadTollManagement a rdfs:Class,
        owl:Class,
        dpv-owl:Purpose ;
    dct:created "2024-12-01"^^xsd:date ;
    rdfs:isDefinedBy sector-infra-owl: ;
    rdfs:subClassOf sector-infra-owl:RoadManagement ;
    sw:term_status "accepted"@en ;
    skos:definition "Purposes associated with management of tolls and other forms of fees for use of road infrastructure"@en ;
    skos:prefLabel "Road Toll Management"@en .

sector-infra-owl:RoadTrafficAnalysis a rdfs:Class,
        owl:Class,
        dpv-owl:Purpose ;
    dct:created "2024-12-01"^^xsd:date ;
    rdfs:isDefinedBy sector-infra-owl: ;
    rdfs:subClassOf sector-infra-owl:RoadResearchDevelopment ;
    sw:term_status "accepted"@en ;
    skos:definition "Purposes associated with analysis of road traffic with the goal of researching and developing improvements to road infrastructure"@en ;
    skos:prefLabel "Road Traffic Analysis"@en .

sector-infra-owl:RoadTrafficManagement a rdfs:Class,
        owl:Class,
        dpv-owl:Purpose ;
    dct:created "2024-12-01"^^xsd:date ;
    rdfs:isDefinedBy sector-infra-owl: ;
    rdfs:subClassOf sector-infra-owl:RoadManagement ;
    sw:term_status "accepted"@en ;
    skos:definition "Purposes associated with management of road traffic"@en ;
    skos:prefLabel "Road Traffic Management"@en .

sector-infra-owl:TransportManagement a rdfs:Class,
        owl:Class,
        dpv-owl:Purpose ;
    dct:created "2024-12-01"^^xsd:date ;
    rdfs:isDefinedBy sector-infra-owl: ;
    rdfs:subClassOf sector-infra-owl:InfrastructureManagement ;
    sw:term_status "accepted"@en ;
    skos:definition "Purposes associated with management of transport infrastructure"@en ;
    skos:prefLabel "Transport Management"@en .

sector-infra-owl:serialisation-html a profile:ResourceDescriptor ;
    dct:conformsTo <https://www.w3.org/TR/html/> ;
    dct:format <https://www.iana.org/assignments/media-types/text/html> ;
    dct:title "Infrastructure Sector Concepts - HTML serialiation" ;
    profile:hasArtifact <https://w3id.org/dpv/sector/infra/sector-infra-owl.html> ;
    profile:hasRole role:specification .

sector-infra-owl:serialisation-jsonld a profile:ResourceDescriptor ;
    dct:conformsTo <https://www.w3.org/TR/json-ld11/> ;
    dct:format <https://www.iana.org/assignments/media-types/application/ld+json> ;
    dct:title "Infrastructure Sector Concepts - JSON-LD serialiation" ;
    profile:hasArtifact <https://w3id.org/dpv/sector/infra/sector-infra-owl.jsonld> ;
    profile:hasRole role:vocabulary .

sector-infra-owl:serialisation-n3 a profile:ResourceDescriptor ;
    dct:conformsTo <https://www.w3.org/TeamSubmission/n3/> ;
    dct:format <https://www.iana.org/assignments/media-types/text/n3> ;
    dct:title "Infrastructure Sector Concepts - N3 serialiation" ;
    profile:hasArtifact <https://w3id.org/dpv/sector/infra/sector-infra-owl.n3> ;
    profile:hasRole role:vocabulary .

sector-infra-owl:serialisation-rdf a profile:ResourceDescriptor ;
    dct:conformsTo rdf: ;
    dct:format <https://www.iana.org/assignments/media-types/application/rdf+xml> ;
    dct:title "Infrastructure Sector Concepts - RDF/XML serialiation" ;
    profile:hasArtifact <https://w3id.org/dpv/sector/infra/sector-infra-owl.rdf> ;
    profile:hasRole role:vocabulary .

sector-infra-owl:serialisation-ttl a profile:ResourceDescriptor ;
    dct:conformsTo <https://www.w3.org/TR/turtle/> ;
    dct:format <https://www.iana.org/assignments/media-types/text/turtle> ;
    dct:title "Infrastructure Sector Concepts - Turtle serialiation" ;
    profile:hasArtifact <https://w3id.org/dpv/sector/infra/sector-infra-owl.ttl> ;
    profile:hasRole role:vocabulary .

<https://w3id.org/dpv/examples> a profile:ResourceDescriptor ;
    dct:conformsTo <https://www.w3.org/TR/html/> ;
    dct:format <https://www.iana.org/assignments/media-types/text/html> ;
    dct:title "Examples for Data Privacy Vocabulary" ;
    profile:hasArtifact <https://w3id.org/dpv/examples> ;
    profile:hasRole role:guidance .

<https://w3id.org/dpv/guides> a profile:ResourceDescriptor ;
    dct:conformsTo <https://www.w3.org/TR/html/> ;
    dct:format <https://www.iana.org/assignments/media-types/text/html> ;
    dct:title "Guides for Data Privacy Vocabulary" ;
    profile:hasArtifact <https://w3id.org/dpv/guides> ;
    profile:hasRole role:guidance .

<https://w3id.org/dpv/primer> a profile:ResourceDescriptor ;
    dct:conformsTo <https://www.w3.org/TR/html/> ;
    dct:format <https://www.iana.org/assignments/media-types/text/html> ;
    dct:title "Primer for Data Privacy Vocabulary" ;
    profile:hasArtifact <https://w3id.org/dpv/primer> ;
    profile:hasRole role:guidance .

sector-infra-owl: a owl:Ontology,
        profile:Profile ;
    dct:bibliographicCitation "Harshvardhan J. Pandit, Beatriz Esteves, Georg P. Krog, Paul Ryan, Delaram Golpayegani, Julian Flake (2025) Data Privacy Vocabulary (DPV) – Version 2.0. In: Demartini, G., et al. The Semantic Web – ISWC 2024. ISWC 2024. Lecture Notes in Computer Science, vol 15233. Springer, Cham. https://doi.org/10.1007/978-3-031-77847-6_10" ;
    dct:conformsTo <http://www.w3.org/2002/07/owl>,
        "http://www.w3.org/2000/01/rdf-schema",
        "http://www.w3.org/2004/02/skos/core" ;
    dct:created "2024-12-01"@en ;
    dct:creator [ a dct:Agent,
                foaf:Person ;
            scoro:hasORCID "0000-0002-5068-3714" ;
            org:memberOf [ a foaf:Organization ;
                    foaf:name "ADAPT Centre, Dublin City University" ] ;
            foaf:homepage "https://harshp.com/" ;
            foaf:name "Harshvardhan J. Pandit" ] ;
    dct:description "Extension to the Data Privacy Vocabulary (DPV) providing concepts for the infrastructure sector"@en ;
    dct:hasVersion sector-infra-owl: ;
    dct:identifier "https://w3id.org/dpv/sector/infra" ;
    dct:issued "2024-12-01"@en ;
    dct:license <https://www.w3.org/copyright/document-license-2023/> ;
    dct:modified "2025-02-01"@en ;
    dct:publisher <https://www.w3.org/> ;
    dct:source <https://www.w3.org/groups/cg/dpvcg/> ;
    dct:title "Infrastructure Sector Concepts"@en ;
    bibo:doi "10.5281/zenodo.12505841" ;
    bibo:status "http://purl.org/ontology/bibo/status/draft" ;
    vann:preferredNamespacePrefix "sector-infra" ;
    vann:preferredNamespaceUri "https://w3id.org/dpv/sector/infra#" ;
    rdfs:Label "SECTOR-INFRA"@en ;
    owl:versionIRI <https://w3id.org/dpv/2.1/sector/infra/owl#> ;
    owl:versionInfo "2.1" ;
    profile:hasResource <https://w3id.org/dpv/examples>,
        <https://w3id.org/dpv/guides>,
        <https://w3id.org/dpv/primer>,
        sector-infra-owl:serialisation-html,
        sector-infra-owl:serialisation-jsonld,
        sector-infra-owl:serialisation-n3,
        sector-infra-owl:serialisation-rdf,
        sector-infra-owl:serialisation-ttl ;
    profile:isProfileOf <http://www.w3.org/2002/07/owl>,
        <https://w3id.org/dpv/owl>,
        sector-infra-owl: ;
    foaf:logo <https://w3id.org/dpv/media/logo.png> ;
    schema:version "2.1" .

