@prefix bibo: <http://purl.org/ontology/bibo/> .
@prefix dcam: <http://purl.org/dc/dcam/> .
@prefix dcat: <http://www.w3.org/ns/dcat#> .
@prefix dct: <http://purl.org/dc/terms/> .
@prefix dex: <https://w3id.org/dpv/examples#> .
@prefix dpv: <https://w3id.org/dpv#> .
@prefix eu-gdpr: <https://w3id.org/dpv/legal/eu/gdpr#> .
@prefix foaf: <http://xmlns.com/foaf/0.1/> .
@prefix justifications: <https://w3id.org/dpv/justifications#> .
@prefix org: <http://www.w3.org/ns/org#> .
@prefix owl: <http://www.w3.org/2002/07/owl#> .
@prefix pd: <https://w3id.org/dpv/pd#> .
@prefix profile: <http://www.w3.org/ns/dx/prof/> .
@prefix rdf: <http://www.w3.org/1999/02/22-rdf-syntax-ns#> .
@prefix rdfs: <http://www.w3.org/2000/01/rdf-schema#> .
@prefix risk: <https://w3id.org/dpv/risk#> .
@prefix role: <http://www.w3.org/ns/dx/prof/role/> .
@prefix schema: <https://schema.org/> .
@prefix scoro: <http://purl.org/spar/scoro/> .
@prefix skos: <http://www.w3.org/2004/02/skos/core#> .
@prefix sw: <http://www.w3.org/2003/06/sw-vocab-status/ns#> .
@prefix vann: <http://purl.org/vocab/vann/> .
@prefix xsd: <http://www.w3.org/2001/XMLSchema#> .

dcat:Resource a rdfs:Class,
        skos:Concept ;
    dct:contributor _:N05cd1f43dbaf4b4ba297dab5ee221394,
        _:N0a43dd9ea5e94fe695d8b7df8802cfdd,
        _:N458008bc6195484e9cc557f70eabda31 ;
    dct:created "2022-11-09"^^xsd:date ;
    rdfs:isDefinedBy eu-gdpr: ;
    skos:inScheme eu-gdpr:rights-classes ;
    skos:prefLabel "dcat:Resource"@en ;
    skos:scopeNote "A dataset or catalogue or any other resource provided in fulfilment of a Right Exercise, such as for GDPR's Art.15 regarding Right of Access or Art.20 regarding Right to Data Portability. The associated properties from DCAT and DCMI DCT vocabularies provide convenient means to express metadata such as URL for accessing the data, its temporal validity and access restrictions, and specific datasets present along with their schemas."@en .

eu-gdpr:A13 a rdfs:Class,
        skos:Concept,
        dpv:Right ;
    dct:contributor _:N05cd1f43dbaf4b4ba297dab5ee221394,
        _:N0a43dd9ea5e94fe695d8b7df8802cfdd,
        _:N458008bc6195484e9cc557f70eabda31 ;
    dct:created "2020-11-04"^^xsd:date ;
    dct:source [ a schema:WebPage ;
            schema:name "GDPR Art.13" ;
            schema:url "https://eur-lex.europa.eu/eli/reg/2016/679/art_13/oj" ] ;
    rdfs:isDefinedBy eu-gdpr: ;
    sw:term_status "accepted"@en ;
    skos:broader dpv:DataSubjectRight ;
    skos:definition "information to be provided where personal data is directly collected from data subject"@en ;
    skos:inScheme eu-gdpr:rights-classes ;
    skos:prefLabel "A13 Right to be Informed"@en ;
    dpv:hasJustification eu-gdpr:JustificationA12LackOfIntent,
        eu-gdpr:JustificationA12MaliciousIntent,
        eu-gdpr:JustificationA12ManifestlyExcessive,
        eu-gdpr:JustificationA12ManifestlyUnfounded,
        eu-gdpr:JustificationA13EntityAlreadyInformed .

eu-gdpr:A13-Denied a rdfs:Class,
        skos:Concept,
        risk:PotentialConsequence,
        risk:PotentialImpact,
        risk:PotentialRisk,
        risk:RiskConcept ;
    dct:created "2024-10-21"^^xsd:date ;
    rdfs:isDefinedBy eu-gdpr: ;
    sw:term_status "accepted"@en ;
    skos:broader eu-gdpr:A13-Impact ;
    skos:definition "A denial that A13 applied to the situation"@en ;
    skos:inScheme eu-gdpr:rights-impacts-classes ;
    skos:prefLabel "A13 Denied"@en .

eu-gdpr:A13-Eroded a rdfs:Class,
        skos:Concept,
        risk:PotentialConsequence,
        risk:PotentialImpact,
        risk:PotentialRisk,
        risk:RiskConcept ;
    dct:created "2024-10-21"^^xsd:date ;
    rdfs:isDefinedBy eu-gdpr: ;
    sw:term_status "accepted"@en ;
    skos:broader eu-gdpr:A13-Impact ;
    skos:definition "Erosion of A13 obligation to provide information e.g. by repeatedly and systematically limited or denying it"@en ;
    skos:inScheme eu-gdpr:rights-impacts-classes ;
    skos:prefLabel "A13 Eroded"@en .

eu-gdpr:A13-ExercisePrevented a rdfs:Class,
        skos:Concept,
        risk:PotentialConsequence,
        risk:PotentialImpact,
        risk:PotentialRisk,
        risk:RiskConcept ;
    dct:created "2024-10-21"^^xsd:date ;
    rdfs:isDefinedBy eu-gdpr: ;
    sw:term_status "accepted"@en ;
    skos:broader eu-gdpr:A13-Impact ;
    skos:definition "The prevention of A13 obligation to provide information e.g. by preventing the data subject from obtaining this information"@en ;
    skos:inScheme eu-gdpr:rights-impacts-classes ;
    skos:prefLabel "A13 ExercisePrevented"@en .

eu-gdpr:A13-Impact a rdfs:Class,
        skos:Concept,
        risk:PotentialConsequence,
        risk:PotentialImpact,
        risk:PotentialRisk,
        risk:RiskConcept ;
    dct:created "2024-10-21"^^xsd:date ;
    dct:source [ a schema:WebPage ;
            schema:name "GDPR Art.13" ;
            schema:url "https://eur-lex.europa.eu/eli/reg/2016/679/art_13/oj" ] ;
    rdfs:isDefinedBy eu-gdpr: ;
    sw:term_status "accepted"@en ;
    skos:broader eu-gdpr:GDPRRightsImpact ;
    skos:definition "Something that acts as or is considered as an impact on A13 Right to be Informed"@en ;
    skos:inScheme eu-gdpr:rights-impacts-classes ;
    skos:prefLabel "Impact on A13 Right to be Informed"@en .

eu-gdpr:A13-Limited a rdfs:Class,
        skos:Concept,
        risk:PotentialConsequence,
        risk:PotentialImpact,
        risk:PotentialRisk,
        risk:RiskConcept ;
    dct:created "2024-10-21"^^xsd:date ;
    rdfs:isDefinedBy eu-gdpr: ;
    sw:term_status "accepted"@en ;
    skos:broader eu-gdpr:A13-Impact ;
    skos:definition "A limited fulfillment of A13 obligation to provide information e.g. not providing all required information"@en ;
    skos:inScheme eu-gdpr:rights-impacts-classes ;
    skos:prefLabel "A13 Limited"@en .

eu-gdpr:A13-Obstructed a rdfs:Class,
        skos:Concept,
        risk:PotentialConsequence,
        risk:PotentialImpact,
        risk:PotentialRisk,
        risk:RiskConcept ;
    dct:created "2024-10-21"^^xsd:date ;
    rdfs:isDefinedBy eu-gdpr: ;
    sw:term_status "accepted"@en ;
    skos:broader eu-gdpr:A13-Impact ;
    skos:definition "Obstruction of A13 obligation to provide information e.g. asking for unnecessary identity verification and making it difficult to obtain information"@en ;
    skos:inScheme eu-gdpr:rights-impacts-classes ;
    skos:prefLabel "A13 Obstructed"@en .

eu-gdpr:A13-Unfulfilled a rdfs:Class,
        skos:Concept,
        risk:PotentialConsequence,
        risk:PotentialImpact,
        risk:PotentialRisk,
        risk:RiskConcept ;
    dct:created "2024-10-21"^^xsd:date ;
    rdfs:isDefinedBy eu-gdpr: ;
    sw:term_status "accepted"@en ;
    skos:broader eu-gdpr:A13-Impact ;
    skos:definition "Non-fulfillment of A13 obligation to provide required information"@en ;
    skos:inScheme eu-gdpr:rights-impacts-classes ;
    skos:prefLabel "A13 Unfulfilled"@en .

eu-gdpr:A13-Violated a rdfs:Class,
        skos:Concept,
        risk:PotentialConsequence,
        risk:PotentialImpact,
        risk:PotentialRisk,
        risk:RiskConcept ;
    dct:created "2024-10-21"^^xsd:date ;
    rdfs:isDefinedBy eu-gdpr: ;
    sw:term_status "accepted"@en ;
    skos:broader eu-gdpr:A13-Impact ;
    skos:definition "A violation of A13 obligation regarding providing information"@en ;
    skos:inScheme eu-gdpr:rights-impacts-classes ;
    skos:prefLabel "A13 Violated"@en ;
    skos:scopeNote "What constitutes as a violation of A13 depends on the particulars of the situation, therefore we suggest first representing the impact using the appropriate category of impact (e.g. denied, limited) and then assessing whether it constitutes as a violation"@en .

eu-gdpr:A14 a rdfs:Class,
        skos:Concept,
        dpv:Right ;
    dct:contributor _:N05cd1f43dbaf4b4ba297dab5ee221394,
        _:N0a43dd9ea5e94fe695d8b7df8802cfdd,
        _:N458008bc6195484e9cc557f70eabda31 ;
    dct:created "2020-11-04"^^xsd:date ;
    dct:source [ a schema:WebPage ;
            schema:name "GDPR Art.14" ;
            schema:url "https://eur-lex.europa.eu/eli/reg/2016/679/art_14/oj" ] ;
    rdfs:isDefinedBy eu-gdpr: ;
    sw:term_status "accepted"@en ;
    skos:broader dpv:DataSubjectRight ;
    skos:definition "information to be provided where personal data is collected from other sources"@en ;
    skos:inScheme eu-gdpr:rights-classes ;
    skos:prefLabel "A14 Right to be Informed"@en ;
    dpv:hasJustification eu-gdpr:JustificationA12IdentityFailure,
        eu-gdpr:JustificationA12IdentityRequired,
        eu-gdpr:JustificationA12InformationRequired,
        eu-gdpr:JustificationA12LackOfIntent,
        eu-gdpr:JustificationA12MaliciousIntent,
        eu-gdpr:JustificationA12ManifestlyExcessive,
        eu-gdpr:JustificationA12ManifestlyUnfounded,
        eu-gdpr:JustificationA14ConfidentialityCompromised,
        eu-gdpr:JustificationA14DisproportionateEffort,
        eu-gdpr:JustificationA14EntityAlreadyInformed,
        eu-gdpr:JustificationA14FulfilmentImpossible,
        eu-gdpr:JustificationA14LegallyExempted,
        eu-gdpr:JustificationA14ObjectivesImpaired .

eu-gdpr:A14-Impact a rdfs:Class,
        skos:Concept,
        risk:PotentialConsequence,
        risk:PotentialImpact,
        risk:PotentialRisk,
        risk:RiskConcept ;
    dct:created "2024-10-21"^^xsd:date ;
    dct:source [ a schema:WebPage ;
            schema:name "GDPR Art.14" ;
            schema:url "https://eur-lex.europa.eu/eli/reg/2016/679/art_14/oj" ] ;
    rdfs:isDefinedBy eu-gdpr: ;
    sw:term_status "accepted"@en ;
    skos:broader eu-gdpr:GDPRRightsImpact ;
    skos:definition "Something that acts as or is considered as an impact on A14 Right to be Informed"@en ;
    skos:inScheme eu-gdpr:rights-impacts-classes ;
    skos:prefLabel "Impact on A14 Right to be Informed"@en .

eu-gdpr:A15 a rdfs:Class,
        skos:Concept,
        dpv:Right ;
    dct:contributor _:N05cd1f43dbaf4b4ba297dab5ee221394,
        _:N0a43dd9ea5e94fe695d8b7df8802cfdd,
        _:N458008bc6195484e9cc557f70eabda31 ;
    dct:created "2020-11-04"^^xsd:date ;
    dct:source [ a schema:WebPage ;
            schema:name "GDPR Art.15" ;
            schema:url "https://eur-lex.europa.eu/eli/reg/2016/679/art_15/oj" ] ;
    rdfs:isDefinedBy eu-gdpr: ;
    sw:term_status "accepted"@en ;
    skos:broader dpv:DataSubjectRight ;
    skos:definition "Right of access"@en ;
    skos:inScheme eu-gdpr:rights-classes ;
    skos:prefLabel "A15 Right of Access"@en ;
    dpv:hasJustification eu-gdpr:JustificationA12Complexity,
        eu-gdpr:JustificationA12Delay,
        eu-gdpr:JustificationA12HighVolume,
        eu-gdpr:JustificationA12IdentityFailure,
        eu-gdpr:JustificationA12IdentityRequired,
        eu-gdpr:JustificationA12InformationRequired,
        eu-gdpr:JustificationA12LackOfIntent,
        eu-gdpr:JustificationA12MaliciousIntent,
        eu-gdpr:JustificationA12ManifestlyExcessive,
        eu-gdpr:JustificationA12ManifestlyUnfounded .

eu-gdpr:A15-Impact a rdfs:Class,
        skos:Concept,
        risk:PotentialConsequence,
        risk:PotentialImpact,
        risk:PotentialRisk,
        risk:RiskConcept ;
    dct:created "2024-10-21"^^xsd:date ;
    dct:source [ a schema:WebPage ;
            schema:name "GDPR Art.15" ;
            schema:url "https://eur-lex.europa.eu/eli/reg/2016/679/art_15/oj" ] ;
    rdfs:isDefinedBy eu-gdpr: ;
    sw:term_status "accepted"@en ;
    skos:broader eu-gdpr:GDPRRightsImpact ;
    skos:definition "Something that acts as or is considered as an impact on A15 Right of Access"@en ;
    skos:inScheme eu-gdpr:rights-impacts-classes ;
    skos:prefLabel "Impact on A15 Right of Access"@en .

eu-gdpr:A16 a rdfs:Class,
        skos:Concept,
        dpv:Right ;
    dct:contributor _:N05cd1f43dbaf4b4ba297dab5ee221394,
        _:N0a43dd9ea5e94fe695d8b7df8802cfdd,
        _:N458008bc6195484e9cc557f70eabda31 ;
    dct:created "2020-11-04"^^xsd:date ;
    dct:source [ a schema:WebPage ;
            schema:name "GDPR Art.16" ;
            schema:url "https://eur-lex.europa.eu/eli/reg/2016/679/art_16/oj" ] ;
    rdfs:isDefinedBy eu-gdpr: ;
    sw:term_status "accepted"@en ;
    skos:broader dpv:DataSubjectRight ;
    skos:definition "Right to rectification"@en ;
    skos:inScheme eu-gdpr:rights-classes ;
    skos:prefLabel "A16 Right to Rectification"@en ;
    dpv:hasJustification eu-gdpr:JustificationA12Complexity,
        eu-gdpr:JustificationA12Delay,
        eu-gdpr:JustificationA12HighVolume,
        eu-gdpr:JustificationA12IdentityFailure,
        eu-gdpr:JustificationA12IdentityRequired,
        eu-gdpr:JustificationA12InformationRequired,
        eu-gdpr:JustificationA12LackOfIntent,
        eu-gdpr:JustificationA12MaliciousIntent,
        eu-gdpr:JustificationA12ManifestlyExcessive,
        eu-gdpr:JustificationA12ManifestlyUnfounded .

eu-gdpr:A16-Impact a rdfs:Class,
        skos:Concept,
        risk:PotentialConsequence,
        risk:PotentialImpact,
        risk:PotentialRisk,
        risk:RiskConcept ;
    dct:created "2024-10-21"^^xsd:date ;
    dct:source [ a schema:WebPage ;
            schema:name "GDPR Art.16" ;
            schema:url "https://eur-lex.europa.eu/eli/reg/2016/679/art_16/oj" ] ;
    rdfs:isDefinedBy eu-gdpr: ;
    sw:term_status "accepted"@en ;
    skos:broader eu-gdpr:GDPRRightsImpact ;
    skos:definition "Something that acts as or is considered as an impact on A16 Right to Rectification"@en ;
    skos:inScheme eu-gdpr:rights-impacts-classes ;
    skos:prefLabel "Impact on A16 Right to Rectification"@en .

eu-gdpr:A17 a rdfs:Class,
        skos:Concept,
        dpv:Right ;
    dct:contributor _:N05cd1f43dbaf4b4ba297dab5ee221394,
        _:N0a43dd9ea5e94fe695d8b7df8802cfdd,
        _:N458008bc6195484e9cc557f70eabda31 ;
    dct:created "2020-11-04"^^xsd:date ;
    dct:source [ a schema:WebPage ;
            schema:name "GDPR Art.17" ;
            schema:url "https://eur-lex.europa.eu/eli/reg/2016/679/art_17/oj" ] ;
    rdfs:isDefinedBy eu-gdpr: ;
    sw:term_status "accepted"@en ;
    skos:broader dpv:DataSubjectRight ;
    skos:definition "Right to erasure ('Right to be forgotten')"@en ;
    skos:inScheme eu-gdpr:rights-classes ;
    skos:prefLabel "A17 Right to Erasure"@en ;
    dpv:hasJustification eu-gdpr:JustificationA12Complexity,
        eu-gdpr:JustificationA12Delay,
        eu-gdpr:JustificationA12HighVolume,
        eu-gdpr:JustificationA12IdentityFailure,
        eu-gdpr:JustificationA12IdentityRequired,
        eu-gdpr:JustificationA12InformationRequired,
        eu-gdpr:JustificationA12LackOfIntent,
        eu-gdpr:JustificationA12MaliciousIntent,
        eu-gdpr:JustificationA12ManifestlyExcessive,
        eu-gdpr:JustificationA12ManifestlyUnfounded,
        eu-gdpr:JustificationA17Archiving,
        eu-gdpr:JustificationA17ChildData,
        eu-gdpr:JustificationA17FreedomOfExpression,
        eu-gdpr:JustificationA17LegalClaims,
        eu-gdpr:JustificationA17LegalErasure,
        eu-gdpr:JustificationA17LegallyRequired,
        eu-gdpr:JustificationA17NoLegalBasis,
        eu-gdpr:JustificationA17NonNecessity,
        eu-gdpr:JustificationA17ObjectA21,
        eu-gdpr:JustificationA17OfficialAuthority,
        eu-gdpr:JustificationA17PublicHealth,
        eu-gdpr:JustificationA17PublicInterest,
        eu-gdpr:JustificationA17UnlawfulProcessing .

eu-gdpr:A17-Impact a rdfs:Class,
        skos:Concept,
        risk:PotentialConsequence,
        risk:PotentialImpact,
        risk:PotentialRisk,
        risk:RiskConcept ;
    dct:created "2024-10-21"^^xsd:date ;
    dct:source [ a schema:WebPage ;
            schema:name "GDPR Art.17" ;
            schema:url "https://eur-lex.europa.eu/eli/reg/2016/679/art_17/oj" ] ;
    rdfs:isDefinedBy eu-gdpr: ;
    sw:term_status "accepted"@en ;
    skos:broader eu-gdpr:GDPRRightsImpact ;
    skos:definition "Something that acts as or is considered as an impact on A17 Right to Erasure"@en ;
    skos:inScheme eu-gdpr:rights-impacts-classes ;
    skos:prefLabel "Impact on A17 Right to Erasure"@en .

eu-gdpr:A18 a rdfs:Class,
        skos:Concept,
        dpv:Right ;
    dct:contributor _:N05cd1f43dbaf4b4ba297dab5ee221394,
        _:N0a43dd9ea5e94fe695d8b7df8802cfdd,
        _:N458008bc6195484e9cc557f70eabda31 ;
    dct:created "2020-11-04"^^xsd:date ;
    dct:source [ a schema:WebPage ;
            schema:name "GDPR Art.18" ;
            schema:url "https://eur-lex.europa.eu/eli/reg/2016/679/art_18/oj" ] ;
    rdfs:isDefinedBy eu-gdpr: ;
    sw:term_status "accepted"@en ;
    skos:broader dpv:DataSubjectRight ;
    skos:definition "Right to restriction of processing"@en ;
    skos:inScheme eu-gdpr:rights-classes ;
    skos:prefLabel "A18 Right to Restrict Processing"@en ;
    dpv:hasJustification eu-gdpr:JustificationA12Complexity,
        eu-gdpr:JustificationA12Delay,
        eu-gdpr:JustificationA12HighVolume,
        eu-gdpr:JustificationA12IdentityFailure,
        eu-gdpr:JustificationA12IdentityRequired,
        eu-gdpr:JustificationA12InformationRequired,
        eu-gdpr:JustificationA12LackOfIntent,
        eu-gdpr:JustificationA12MaliciousIntent,
        eu-gdpr:JustificationA12ManifestlyExcessive,
        eu-gdpr:JustificationA12ManifestlyUnfounded .

eu-gdpr:A18-Impact a rdfs:Class,
        skos:Concept,
        risk:PotentialConsequence,
        risk:PotentialImpact,
        risk:PotentialRisk,
        risk:RiskConcept ;
    dct:created "2024-10-21"^^xsd:date ;
    dct:source [ a schema:WebPage ;
            schema:name "GDPR Art.18" ;
            schema:url "https://eur-lex.europa.eu/eli/reg/2016/679/art_18/oj" ] ;
    rdfs:isDefinedBy eu-gdpr: ;
    sw:term_status "accepted"@en ;
    skos:broader eu-gdpr:GDPRRightsImpact ;
    skos:definition "Something that acts as or is considered as an impact on A18 Right to Restrict Processing"@en ;
    skos:inScheme eu-gdpr:rights-impacts-classes ;
    skos:prefLabel "Impact on A18 Right to Restrict Processing"@en .

eu-gdpr:A19 a rdfs:Class,
        skos:Concept,
        dpv:Right ;
    dct:contributor _:N05cd1f43dbaf4b4ba297dab5ee221394,
        _:N0a43dd9ea5e94fe695d8b7df8802cfdd,
        _:N458008bc6195484e9cc557f70eabda31 ;
    dct:created "2020-11-04"^^xsd:date ;
    dct:modified "2024-04-14"^^xsd:date ;
    dct:source [ a schema:WebPage ;
            schema:name "GDPR Art.19" ;
            schema:url "https://eur-lex.europa.eu/eli/reg/2016/679/art_19/oj" ] ;
    rdfs:isDefinedBy eu-gdpr: ;
    sw:term_status "accepted"@en ;
    skos:broader dpv:DataSubjectRight ;
    skos:definition "Right to be notified in case of rectification or erasure of personal data or restriction of processing"@en ;
    skos:inScheme eu-gdpr:rights-classes ;
    skos:prefLabel "A19 Right to Rectification Notification"@en ;
    dpv:hasJustification eu-gdpr:JustificationA12Complexity,
        eu-gdpr:JustificationA12Delay,
        eu-gdpr:JustificationA12HighVolume,
        eu-gdpr:JustificationA12IdentityFailure,
        eu-gdpr:JustificationA12IdentityRequired,
        eu-gdpr:JustificationA12InformationRequired,
        eu-gdpr:JustificationA12LackOfIntent,
        eu-gdpr:JustificationA12MaliciousIntent,
        eu-gdpr:JustificationA12ManifestlyExcessive,
        eu-gdpr:JustificationA12ManifestlyUnfounded .

eu-gdpr:A19-Impact a rdfs:Class,
        skos:Concept,
        risk:PotentialConsequence,
        risk:PotentialImpact,
        risk:PotentialRisk,
        risk:RiskConcept ;
    dct:created "2024-10-21"^^xsd:date ;
    dct:source [ a schema:WebPage ;
            schema:name "GDPR Art.19" ;
            schema:url "https://eur-lex.europa.eu/eli/reg/2016/679/art_19/oj" ] ;
    rdfs:isDefinedBy eu-gdpr: ;
    sw:term_status "accepted"@en ;
    skos:broader eu-gdpr:GDPRRightsImpact ;
    skos:definition "Something that acts as or is considered as an impact on A19 Right to Rectification Notification"@en ;
    skos:inScheme eu-gdpr:rights-impacts-classes ;
    skos:prefLabel "Impact on A19 Right to Rectification Notification"@en .

eu-gdpr:A20 a rdfs:Class,
        skos:Concept,
        dpv:Right ;
    dct:contributor _:N05cd1f43dbaf4b4ba297dab5ee221394,
        _:N0a43dd9ea5e94fe695d8b7df8802cfdd,
        _:N458008bc6195484e9cc557f70eabda31 ;
    dct:created "2020-11-04"^^xsd:date ;
    dct:source [ a schema:WebPage ;
            schema:name "GDPR Art.20" ;
            schema:url "https://eur-lex.europa.eu/eli/reg/2016/679/art_20/oj" ] ;
    rdfs:isDefinedBy eu-gdpr: ;
    sw:term_status "accepted"@en ;
    skos:broader dpv:DataSubjectRight ;
    skos:definition "Right to data portability"@en ;
    skos:inScheme eu-gdpr:rights-classes ;
    skos:prefLabel "A20 Right to Data Portability"@en ;
    dpv:hasJustification eu-gdpr:JustificationA12Complexity,
        eu-gdpr:JustificationA12Delay,
        eu-gdpr:JustificationA12HighVolume,
        eu-gdpr:JustificationA12IdentityFailure,
        eu-gdpr:JustificationA12IdentityRequired,
        eu-gdpr:JustificationA12InformationRequired,
        eu-gdpr:JustificationA12LackOfIntent,
        eu-gdpr:JustificationA12MaliciousIntent,
        eu-gdpr:JustificationA12ManifestlyExcessive,
        eu-gdpr:JustificationA12ManifestlyUnfounded .

eu-gdpr:A20-Impact a rdfs:Class,
        skos:Concept,
        risk:PotentialConsequence,
        risk:PotentialImpact,
        risk:PotentialRisk,
        risk:RiskConcept ;
    dct:created "2024-10-21"^^xsd:date ;
    dct:source [ a schema:WebPage ;
            schema:name "GDPR Art.20" ;
            schema:url "https://eur-lex.europa.eu/eli/reg/2016/679/art_20/oj" ] ;
    rdfs:isDefinedBy eu-gdpr: ;
    sw:term_status "accepted"@en ;
    skos:broader eu-gdpr:GDPRRightsImpact ;
    skos:definition "Something that acts as or is considered as an impact on A20 Right to Data Portability"@en ;
    skos:inScheme eu-gdpr:rights-impacts-classes ;
    skos:prefLabel "Impact on A20 Right to Data Portability"@en .

eu-gdpr:A21 a rdfs:Class,
        skos:Concept,
        dpv:Right ;
    dct:contributor _:N05cd1f43dbaf4b4ba297dab5ee221394,
        _:N0a43dd9ea5e94fe695d8b7df8802cfdd,
        _:N458008bc6195484e9cc557f70eabda31 ;
    dct:created "2020-11-04"^^xsd:date ;
    dct:source [ a schema:WebPage ;
            schema:name "GDPR Art.21" ;
            schema:url "https://eur-lex.europa.eu/eli/reg/2016/679/art_21/oj" ] ;
    rdfs:isDefinedBy eu-gdpr: ;
    sw:term_status "accepted"@en ;
    skos:broader dpv:DataSubjectRight ;
    skos:definition "Right to object to processing of personal data"@en ;
    skos:inScheme eu-gdpr:rights-classes ;
    skos:prefLabel "A21 Right to object"@en ;
    dpv:hasJustification eu-gdpr:JustificationA12Complexity,
        eu-gdpr:JustificationA12Delay,
        eu-gdpr:JustificationA12HighVolume,
        eu-gdpr:JustificationA12IdentityFailure,
        eu-gdpr:JustificationA12IdentityRequired,
        eu-gdpr:JustificationA12InformationRequired,
        eu-gdpr:JustificationA12LackOfIntent,
        eu-gdpr:JustificationA12MaliciousIntent,
        eu-gdpr:JustificationA12ManifestlyExcessive,
        eu-gdpr:JustificationA12ManifestlyUnfounded .

eu-gdpr:A21-Impact a rdfs:Class,
        skos:Concept,
        risk:PotentialConsequence,
        risk:PotentialImpact,
        risk:PotentialRisk,
        risk:RiskConcept ;
    dct:created "2024-10-21"^^xsd:date ;
    dct:source [ a schema:WebPage ;
            schema:name "GDPR Art.21" ;
            schema:url "https://eur-lex.europa.eu/eli/reg/2016/679/art_21/oj" ] ;
    rdfs:isDefinedBy eu-gdpr: ;
    sw:term_status "accepted"@en ;
    skos:broader eu-gdpr:GDPRRightsImpact ;
    skos:definition "Something that acts as or is considered as an impact on A21 Right to object"@en ;
    skos:inScheme eu-gdpr:rights-impacts-classes ;
    skos:prefLabel "Impact on A21 Right to object"@en .

eu-gdpr:A22 a rdfs:Class,
        skos:Concept,
        dpv:Right ;
    dct:contributor _:N05cd1f43dbaf4b4ba297dab5ee221394,
        _:N0a43dd9ea5e94fe695d8b7df8802cfdd,
        _:N458008bc6195484e9cc557f70eabda31 ;
    dct:created "2020-11-04"^^xsd:date ;
    dct:modified "2024-12-17"^^xsd:date ;
    dct:source [ a schema:WebPage ;
            schema:name "GDPR Art.22" ;
            schema:url "https://eur-lex.europa.eu/eli/reg/2016/679/art_22/oj" ] ;
    rdfs:isDefinedBy eu-gdpr: ;
    sw:term_status "modified"@en ;
    skos:broader dpv:DataSubjectRight ;
    skos:definition "Right not to be subject to a decision based solely on automated processing including profiling, and for the data subject to obtain human intervention on the part of the controller for the contested or objected activity, and for the data subject to express his or her point of view, and for the data subject to contest the decision"@en ;
    skos:inScheme eu-gdpr:rights-classes ;
    skos:prefLabel "A22 Right to object to automated decision making"@en ;
    dpv:hasJustification eu-gdpr:JustificationA12Complexity,
        eu-gdpr:JustificationA12Delay,
        eu-gdpr:JustificationA12HighVolume,
        eu-gdpr:JustificationA12LackOfIntent,
        eu-gdpr:JustificationA12MaliciousIntent,
        eu-gdpr:JustificationA12ManifestlyExcessive,
        eu-gdpr:JustificationA12ManifestlyUnfounded .

eu-gdpr:A22-3-a a rdfs:Class,
        skos:Concept,
        dpv:Right ;
    dct:contributor _:N05cd1f43dbaf4b4ba297dab5ee221394,
        _:N0a43dd9ea5e94fe695d8b7df8802cfdd,
        _:N458008bc6195484e9cc557f70eabda31 ;
    dct:created "2020-11-04"^^xsd:date ;
    dct:modified "2024-12-17"^^xsd:date ;
    dct:source [ a schema:WebPage ;
            schema:name "GDPR Art.22" ;
            schema:url "https://eur-lex.europa.eu/eli/reg/2016/679/art_22/oj" ] ;
    rdfs:isDefinedBy eu-gdpr: ;
    sw:term_status "modified"@en ;
    skos:broader eu-gdpr:A22 ;
    skos:definition "Right of the data subject to obtain human intervention on the part of the controller for the contested or objected activity"@en ;
    skos:inScheme eu-gdpr:rights-classes ;
    skos:prefLabel "A22 Right to human intervention"@en .

eu-gdpr:A22-3-b a rdfs:Class,
        skos:Concept,
        dpv:Right ;
    dct:contributor _:N05cd1f43dbaf4b4ba297dab5ee221394,
        _:N0a43dd9ea5e94fe695d8b7df8802cfdd,
        _:N458008bc6195484e9cc557f70eabda31 ;
    dct:created "2020-11-04"^^xsd:date ;
    dct:modified "2024-12-17"^^xsd:date ;
    dct:source [ a schema:WebPage ;
            schema:name "GDPR Art.22" ;
            schema:url "https://eur-lex.europa.eu/eli/reg/2016/679/art_22/oj" ] ;
    rdfs:isDefinedBy eu-gdpr: ;
    sw:term_status "modified"@en ;
    skos:broader eu-gdpr:A22 ;
    skos:definition "Right of the data subject to express his or her point of view"@en ;
    skos:inScheme eu-gdpr:rights-classes ;
    skos:prefLabel "A22 Right to express point of view"@en .

eu-gdpr:A22-3-c a rdfs:Class,
        skos:Concept,
        dpv:Right ;
    dct:contributor _:N05cd1f43dbaf4b4ba297dab5ee221394,
        _:N0a43dd9ea5e94fe695d8b7df8802cfdd,
        _:N458008bc6195484e9cc557f70eabda31 ;
    dct:created "2020-11-04"^^xsd:date ;
    dct:modified "2024-12-17"^^xsd:date ;
    dct:source [ a schema:WebPage ;
            schema:name "GDPR Art.22" ;
            schema:url "https://eur-lex.europa.eu/eli/reg/2016/679/art_22/oj" ] ;
    rdfs:isDefinedBy eu-gdpr: ;
    sw:term_status "modified"@en ;
    skos:broader eu-gdpr:A22 ;
    skos:definition "Right of the data subject to contest the decision"@en ;
    skos:inScheme eu-gdpr:rights-classes ;
    skos:prefLabel "A22 Right to contest decision"@en .

eu-gdpr:A22-Impact a rdfs:Class,
        skos:Concept,
        risk:PotentialConsequence,
        risk:PotentialImpact,
        risk:PotentialRisk,
        risk:RiskConcept ;
    dct:created "2024-10-21"^^xsd:date ;
    dct:source [ a schema:WebPage ;
            schema:name "GDPR Art.22" ;
            schema:url "https://eur-lex.europa.eu/eli/reg/2016/679/art_22/oj" ] ;
    rdfs:isDefinedBy eu-gdpr: ;
    sw:term_status "accepted"@en ;
    skos:broader eu-gdpr:GDPRRightsImpact ;
    skos:definition "Something that acts as or is considered as an impact on A22 Right to object to automated decision making"@en ;
    skos:inScheme eu-gdpr:rights-impacts-classes ;
    skos:prefLabel "Impact on A22 Right to object to automated decision making"@en .

eu-gdpr:A45-3 a rdfs:Class,
        skos:Concept,
        dpv:LegalBasis ;
    dct:contributor _:N05cd1f43dbaf4b4ba297dab5ee221394 ;
    dct:created "2020-11-04"^^xsd:date ;
    dct:modified "2021-09-08"^^xsd:date ;
    dct:source [ a schema:WebPage ;
            schema:name "GDPR Art.45-3" ;
            schema:url "https://eur-lex.europa.eu/eli/reg/2016/679/art_45/par_3/oj" ] ;
    rdfs:isDefinedBy eu-gdpr: ;
    sw:term_status "accepted"@en ;
    skos:broader dpv:DataTransferLegalBasis ;
    skos:definition "Personal data can flow freely from the EU to a third country with an Adequacy Decision without any further safeguard being necessary."@en ;
    skos:inScheme eu-gdpr:legal-basis-data-transfer-classes ;
    skos:prefLabel "Art 45(3) adequacy decision"@en ;
    skos:scopeNote "Transfer from EU to a third country. Third country has Adequacy Decision."@en .

eu-gdpr:A46-2-a a rdfs:Class,
        skos:Concept,
        dpv:LegalBasis ;
    dct:contributor _:N05cd1f43dbaf4b4ba297dab5ee221394 ;
    dct:created "2020-11-04"^^xsd:date ;
    dct:modified "2021-09-08"^^xsd:date ;
    dct:source [ a schema:WebPage ;
            schema:name "GDPR Art.46-2a" ;
            schema:url "https://eur-lex.europa.eu/eli/reg/2016/679/art_46/par_2/pnt_a/oj" ] ;
    rdfs:isDefinedBy eu-gdpr: ;
    sw:term_status "accepted"@en ;
    skos:broader dpv:DataTransferLegalBasis ;
    skos:definition "A legally binding and enforceable instrument between public authorities or bodies"@en ;
    skos:inScheme eu-gdpr:legal-basis-data-transfer-classes ;
    skos:prefLabel "Art 46(2-a) legal instrument"@en ;
    skos:scopeNote "Transfer from EU to a third country. Third country has no Adequacy Decision. Third country has appropriate safeguards. Transfer does not require specific authorisation from a Supervisor Authority."@en .

eu-gdpr:A46-2-b a rdfs:Class,
        skos:Concept,
        dpv:LegalBasis ;
    dct:contributor _:N05cd1f43dbaf4b4ba297dab5ee221394 ;
    dct:created "2020-11-04"^^xsd:date ;
    dct:modified "2021-09-08"^^xsd:date ;
    dct:source [ a schema:WebPage ;
            schema:name "GDPR Art.46-2b" ;
            schema:url "https://eur-lex.europa.eu/eli/reg/2016/679/art_46/par_2/pnt_b/oj" ] ;
    rdfs:isDefinedBy eu-gdpr: ;
    sw:term_status "accepted"@en ;
    skos:broader dpv:DataTransferLegalBasis,
        eu-gdpr:BindingCorporateRules ;
    skos:definition "‘Binding Corporate Rules’ means personal data protection policies which are adhered to by a controller or processor established on the territory of a Member State for transfers or a set of transfers of personal data to a controller or processor in one or more third countries within a group of undertakings, or group of enterprises engaged in a joint economic activity"@en ;
    skos:inScheme eu-gdpr:legal-basis-data-transfer-classes ;
    skos:prefLabel "Art 46(2-b) Binding Corporate Rules (BCR)"@en ;
    skos:scopeNote "Transfer from EU to a third country. Third country has no Adequacy Decision. Third country has appropriate safeguards. Transfer does not require specific authorisation from a Supervisor Authority."@en .

eu-gdpr:A46-2-c a rdfs:Class,
        skos:Concept,
        dpv:LegalBasis ;
    dct:contributor _:N05cd1f43dbaf4b4ba297dab5ee221394 ;
    dct:created "2020-11-04"^^xsd:date ;
    dct:modified "2021-09-08"^^xsd:date ;
    dct:source [ a schema:WebPage ;
            schema:name "GDPR Art.46-2c" ;
            schema:url "https://eur-lex.europa.eu/eli/reg/2016/679/art_46/par_2/pnt_c/oj" ] ;
    rdfs:isDefinedBy eu-gdpr: ;
    sw:term_status "accepted"@en ;
    skos:broader dpv:DataTransferLegalBasis,
        eu-gdpr:SCCByCommission ;
    skos:definition "Standard data protection clauses adopted by the Commission"@en ;
    skos:inScheme eu-gdpr:legal-basis-data-transfer-classes ;
    skos:prefLabel "Art 46(2-c) Standard Contractual Clauses (SCC) by EC"@en ;
    skos:scopeNote "Transfer from EU to a third country. Third country has no Adequacy Decision. Third country has appropriate safeguards. Transfer does not require specific authorisation from a Supervisor Authority."@en .

eu-gdpr:A46-2-d a rdfs:Class,
        skos:Concept,
        dpv:LegalBasis ;
    dct:contributor _:N05cd1f43dbaf4b4ba297dab5ee221394 ;
    dct:created "2020-11-04"^^xsd:date ;
    dct:modified "2021-09-08"^^xsd:date ;
    dct:source [ a schema:WebPage ;
            schema:name "GDPR Art.46-2d" ;
            schema:url "https://eur-lex.europa.eu/eli/reg/2016/679/art_46/par_2/pnt_d/oj" ] ;
    rdfs:isDefinedBy eu-gdpr: ;
    sw:term_status "accepted"@en ;
    skos:broader dpv:DataTransferLegalBasis,
        eu-gdpr:SCCBySupervisoryAuthority ;
    skos:definition "Standard data protection clauses adopted by a Supervisory Authority"@en ;
    skos:inScheme eu-gdpr:legal-basis-data-transfer-classes ;
    skos:prefLabel "Art 46(2-d) Standard Contractual Clauses (SCC) by DPA"@en ;
    skos:scopeNote "Transfer from EU to a third country. Third country has no Adequacy Decision. Third country has appropriate safeguards. Transfer does not require specific authorisation from a Supervisor Authority"@en .

eu-gdpr:A46-2-e a rdfs:Class,
        skos:Concept,
        dpv:LegalBasis ;
    dct:contributor _:N05cd1f43dbaf4b4ba297dab5ee221394 ;
    dct:created "2020-11-04"^^xsd:date ;
    dct:modified "2021-09-08"^^xsd:date ;
    dct:source [ a schema:WebPage ;
            schema:name "GDPR Art.46-2e" ;
            schema:url "https://eur-lex.europa.eu/eli/reg/2016/679/art_46/par_2/pnt_e/oj" ] ;
    rdfs:isDefinedBy eu-gdpr: ;
    sw:term_status "accepted"@en ;
    skos:broader dpv:DataTransferLegalBasis ;
    skos:definition "An approved code of conduct pursuant to GDPR Article 40 together with binding and enforceable commitments of the controller or processor in the third country to apply the appropriate safeguards, including as regards individuals´ rights"@en ;
    skos:inScheme eu-gdpr:legal-basis-data-transfer-classes ;
    skos:prefLabel "Art 46(2-e) code of conduct"@en ;
    skos:scopeNote "Transfer from EU to a third country. Third country has no Adequacy Decision. Third country has appropriate safeguards. Transfer does not require specific authorisation from a Supervisor Authority."@en .

eu-gdpr:A46-2-f a rdfs:Class,
        skos:Concept,
        dpv:LegalBasis ;
    dct:contributor _:N05cd1f43dbaf4b4ba297dab5ee221394 ;
    dct:created "2020-11-04"^^xsd:date ;
    dct:modified "2021-09-08"^^xsd:date ;
    dct:source [ a schema:WebPage ;
            schema:name "GDPR Art.46-2f" ;
            schema:url "https://eur-lex.europa.eu/eli/reg/2016/679/art_46/par_2/pnt_f/oj" ] ;
    rdfs:isDefinedBy eu-gdpr: ;
    sw:term_status "accepted"@en ;
    skos:broader dpv:DataTransferLegalBasis ;
    skos:definition "An approved certification mechanism pursuant to GDPR Article 42 together with binding and enforceable commitments of the controller or processor in the third country to apply the appropriate safeguards, including as regards individuals` rights"@en ;
    skos:inScheme eu-gdpr:legal-basis-data-transfer-classes ;
    skos:prefLabel "Art 46(2-f) certification"@en ;
    skos:scopeNote "Transfer from EU to a third country. Third country has no Adequacy Decision. Third country has appropriate safeguards. Transfer does not require specific authorisation from a Supervisor Authority."@en .

eu-gdpr:A46-3-a a rdfs:Class,
        skos:Concept,
        dpv:LegalBasis ;
    dct:contributor _:N05cd1f43dbaf4b4ba297dab5ee221394 ;
    dct:created "2020-11-04"^^xsd:date ;
    dct:modified "2021-09-08"^^xsd:date ;
    dct:source [ a schema:WebPage ;
            schema:name "GDPR Art.46-3a" ;
            schema:url "https://eur-lex.europa.eu/eli/reg/2016/679/art_46/par_3/pnt_a/oj" ] ;
    rdfs:isDefinedBy eu-gdpr: ;
    sw:term_status "accepted"@en ;
    skos:broader dpv:DataTransferLegalBasis ;
    skos:definition "Contractual clauses with controller, processor or recipient of the personal data in the third country or the international organisation."@en ;
    skos:inScheme eu-gdpr:legal-basis-data-transfer-classes ;
    skos:prefLabel "Art 46(3-a) contractual clauses"@en ;
    skos:scopeNote "Transfer from EU to a third country. Third country has no Adequacy Decision. Appropriate safeguards exist. Transfer does requires specific authorisation from a Supervisor Authority."@en .

eu-gdpr:A46-3-b a rdfs:Class,
        skos:Concept,
        dpv:LegalBasis ;
    dct:contributor _:N05cd1f43dbaf4b4ba297dab5ee221394 ;
    dct:created "2020-11-04"^^xsd:date ;
    dct:modified "2021-09-08"^^xsd:date ;
    dct:source [ a schema:WebPage ;
            schema:name "GDPR Art.46-3b" ;
            schema:url "https://eur-lex.europa.eu/eli/reg/2016/679/art_46/par_3/pnt_b/oj" ] ;
    rdfs:isDefinedBy eu-gdpr: ;
    sw:term_status "accepted"@en ;
    skos:broader dpv:DataTransferLegalBasis ;
    skos:definition "Provisions to be inserted into administrative arrangements between public authorities or bodies which include enforceable and effective data subject rights"@en ;
    skos:inScheme eu-gdpr:legal-basis-data-transfer-classes ;
    skos:prefLabel "Art 46(3-b) administrative arrangements"@en ;
    skos:scopeNote "Transfer from EU to a third country. Third country has no Adequacy Decision. Appropriate safeguards exist. Transfer does requires specific authorisation from a Supervisor Authority."@en .

eu-gdpr:A49-1-a a rdfs:Class,
        skos:Concept,
        dpv:LegalBasis ;
    dct:contributor _:N05cd1f43dbaf4b4ba297dab5ee221394 ;
    dct:created "2020-11-04"^^xsd:date ;
    dct:modified "2024-12-17"^^xsd:date ;
    dct:source [ a schema:WebPage ;
            schema:name "GDPR Art.49-1a" ;
            schema:url "https://eur-lex.europa.eu/eli/reg/2016/679/art_49/par_1/pnt_a/oj" ] ;
    rdfs:isDefinedBy eu-gdpr: ;
    sw:term_status "modified"@en ;
    skos:broader dpv:DataTransferLegalBasis,
        dpv:ExplicitlyExpressedConsent,
        eu-gdpr:Consent ;
    skos:definition "The data subject has explicitly consented to the proposed transfer, after having been informed of the possible risks of such transfers for the data subject due to the absence of an adequacy decision and appropriate safeguards."@en ;
    skos:inScheme eu-gdpr:legal-basis-data-transfer-classes ;
    skos:prefLabel "Art 49(1-a) explicit consent"@en ;
    skos:scopeNote "Transfer from EU to a third country. Third country has no Adequacy Decision. Appropriate safeguards do not exist."@en .

eu-gdpr:A49-1-b a rdfs:Class,
        skos:Concept,
        dpv:LegalBasis ;
    dct:contributor _:N05cd1f43dbaf4b4ba297dab5ee221394 ;
    dct:created "2020-11-04"^^xsd:date ;
    dct:modified "2021-09-08"^^xsd:date ;
    dct:source [ a schema:WebPage ;
            schema:name "GDPR Art.49-1b" ;
            schema:url "https://eur-lex.europa.eu/eli/reg/2016/679/art_49/par_1/pnt_b/oj" ] ;
    rdfs:isDefinedBy eu-gdpr: ;
    sw:term_status "accepted"@en ;
    skos:broader dpv:Contract,
        dpv:DataTransferLegalBasis ;
    skos:definition "The transfer is necessary for the performance of a contract between the data subject and controller or the implementation of pre-contractual measures taken at the data subject´s request."@en ;
    skos:inScheme eu-gdpr:legal-basis-data-transfer-classes ;
    skos:prefLabel "Art 49(1-b) performance of contract"@en ;
    skos:scopeNote "Transfer from EU to a third country. Third country has no Adequacy Decision. Appropriate safeguards do not exist."@en .

eu-gdpr:A49-1-c a rdfs:Class,
        skos:Concept,
        dpv:LegalBasis ;
    dct:contributor _:N05cd1f43dbaf4b4ba297dab5ee221394 ;
    dct:created "2020-11-04"^^xsd:date ;
    dct:modified "2021-09-08"^^xsd:date ;
    dct:source [ a schema:WebPage ;
            schema:name "GDPR Art.49-1c" ;
            schema:url "https://eur-lex.europa.eu/eli/reg/2016/679/art_49/par_1/pnt_c/oj" ] ;
    rdfs:isDefinedBy eu-gdpr: ;
    sw:term_status "accepted"@en ;
    skos:broader dpv:Contract,
        dpv:DataTransferLegalBasis ;
    skos:definition "The transfer is necessary for the conclusion or performance of a contract concluded in the interest of the data subject and controller and another natural or legal person."@en ;
    skos:inScheme eu-gdpr:legal-basis-data-transfer-classes ;
    skos:prefLabel "Art 49(1-c) conclusion of contract"@en ;
    skos:scopeNote "Transfer from EU to a third country. Third country has no Adequacy Decision. Appropriate safeguards do not exist."@en .

eu-gdpr:A49-1-d a rdfs:Class,
        skos:Concept,
        dpv:LegalBasis ;
    dct:contributor _:N05cd1f43dbaf4b4ba297dab5ee221394 ;
    dct:created "2020-11-04"^^xsd:date ;
    dct:modified "2021-09-08"^^xsd:date ;
    dct:source [ a schema:WebPage ;
            schema:name "GDPR Art.49-1d" ;
            schema:url "https://eur-lex.europa.eu/eli/reg/2016/679/art_49/par_1/pnt_d/oj" ] ;
    rdfs:isDefinedBy eu-gdpr: ;
    sw:term_status "accepted"@en ;
    skos:broader dpv:DataTransferLegalBasis,
        dpv:PublicInterest ;
    skos:definition "The transfer is necessary for important reasons of public interest."@en ;
    skos:inScheme eu-gdpr:legal-basis-data-transfer-classes ;
    skos:prefLabel "Art 49(1-d) public interest"@en ;
    skos:scopeNote "Transfer from EU to a third country. Third country has no Adequacy Decision. Appropriate safeguards do not exist."@en .

eu-gdpr:A49-1-e a rdfs:Class,
        skos:Concept,
        dpv:LegalBasis ;
    dct:contributor _:N05cd1f43dbaf4b4ba297dab5ee221394 ;
    dct:created "2020-11-04"^^xsd:date ;
    dct:modified "2021-09-08"^^xsd:date ;
    dct:source [ a schema:WebPage ;
            schema:name "GDPR Art.49-1e" ;
            schema:url "https://eur-lex.europa.eu/eli/reg/2016/679/art_49/par_1/pnt_e/oj" ] ;
    rdfs:isDefinedBy eu-gdpr: ;
    sw:term_status "accepted"@en ;
    skos:broader dpv:DataTransferLegalBasis ;
    skos:definition "The transfer is necessary for the establishment, exercise or defence of legal claims."@en ;
    skos:inScheme eu-gdpr:legal-basis-data-transfer-classes ;
    skos:prefLabel "Art 49(1-e) legal claims"@en ;
    skos:scopeNote "Transfer from EU to a third country. Third country has no Adequacy Decision. Appropriate safeguards do not exist."@en .

eu-gdpr:A49-1-f a rdfs:Class,
        skos:Concept,
        dpv:LegalBasis ;
    dct:contributor _:N05cd1f43dbaf4b4ba297dab5ee221394 ;
    dct:created "2020-11-04"^^xsd:date ;
    dct:modified "2021-09-08"^^xsd:date ;
    dct:source [ a schema:WebPage ;
            schema:name "GDPR Art.49-1f" ;
            schema:url "https://eur-lex.europa.eu/eli/reg/2016/679/art_49/par_1/pnt_f/oj" ] ;
    rdfs:isDefinedBy eu-gdpr: ;
    sw:term_status "accepted"@en ;
    skos:broader dpv:DataTransferLegalBasis,
        dpv:VitalInterestOfNaturalPerson ;
    skos:definition "The transfer is necessary in order to protect the vital interests of the data subject or of other persons, where the person is physically or legally incapable of giving consent."@en ;
    skos:inScheme eu-gdpr:legal-basis-data-transfer-classes ;
    skos:prefLabel "Art 49(1-f) protect vital interests"@en ;
    skos:scopeNote "Transfer from EU to a third country. Third country has no Adequacy Decision. Appropriate safeguards do not exist."@en .

eu-gdpr:A49-1-g a rdfs:Class,
        skos:Concept,
        dpv:LegalBasis ;
    dct:contributor _:N05cd1f43dbaf4b4ba297dab5ee221394 ;
    dct:created "2020-11-04"^^xsd:date ;
    dct:modified "2021-09-08"^^xsd:date ;
    dct:source [ a schema:WebPage ;
            schema:name "GDPR Art.49-1g" ;
            schema:url "https://eur-lex.europa.eu/eli/reg/2016/679/art_49/par_1/pnt_g/oj" ] ;
    rdfs:isDefinedBy eu-gdpr: ;
    sw:term_status "accepted"@en ;
    skos:broader dpv:DataTransferLegalBasis ;
    skos:definition "The transfer is made from a register which according to Union or Member State law is intended to provide information to the public in general or by any person who can demonstrate a legitimate interest, but only to the extent that the conditions laid down by Union or Member State law for consultation are fulfilled in the particular case."@en ;
    skos:inScheme eu-gdpr:legal-basis-data-transfer-classes ;
    skos:prefLabel "Art 49(1-g) public register"@en ;
    skos:scopeNote "Transfer from EU to a third country. Third country has not Adequacy Decision. Appropriate safeguards do not exist."@en .

eu-gdpr:A49-2 a rdfs:Class,
        skos:Concept,
        dpv:LegalBasis ;
    dct:contributor _:N05cd1f43dbaf4b4ba297dab5ee221394 ;
    dct:created "2020-11-04"^^xsd:date ;
    dct:modified "2021-09-08"^^xsd:date ;
    dct:source [ a schema:WebPage ;
            schema:name "GDPR Art.49-2" ;
            schema:url "https://eur-lex.europa.eu/eli/reg/2016/679/art_49/par_2/oj" ] ;
    rdfs:isDefinedBy eu-gdpr: ;
    sw:term_status "accepted"@en ;
    skos:broader dpv:DataTransferLegalBasis,
        dpv:LegitimateInterest ;
    skos:definition "The transfer is not repetitive, concerns only a limited number of data subjects, is necessary for the purposes of compelling legitimate interests pursued by controller which are not overridden by the interests or rights and freedoms of the data subject, and controller has assessed all the circumstances surrounding the data transfer and have on the basis of that assessment provided suitable safeguards with regard to the protection of personal data."@en ;
    skos:inScheme eu-gdpr:legal-basis-data-transfer-classes ;
    skos:prefLabel "Art 49(2) legitimate interests"@en ;
    skos:scopeNote "Transfer from EU to a third country. Third country has no Adequacy Decision. Appropriate safeguards do not exist and no other options apply."@en .

eu-gdpr:A6-1-a a rdfs:Class,
        skos:Concept,
        dpv:LegalBasis ;
    dct:contributor _:N0a43dd9ea5e94fe695d8b7df8802cfdd ;
    dct:created "2022-09-07"^^xsd:date ;
    dct:modified "2024-12-17"^^xsd:date ;
    dct:source [ a schema:WebPage ;
            schema:name "GDPR Art.6-1a" ;
            schema:url "https://eur-lex.europa.eu/eli/reg/2016/679/art_6/par_1/pnt_a/oj" ] ;
    rdfs:isDefinedBy eu-gdpr: ;
    sw:term_status "modified"@en ;
    skos:broader dpv:ExpressedConsent,
        eu-gdpr:Consent ;
    skos:definition "Legal basis based on data subject's given consent to the processing of his or her personal data for one or more specific purposes"@en ;
    skos:inScheme eu-gdpr:legal-basis-classes ;
    skos:prefLabel "Art.6(1-a) consent"@en ;
    skos:scopeNote "Consent can be explicit or non-explicit. To express these specifically, see the explicit and non-explicit variations provided for Art.6-1a."@en ;
    dpv:hasRight eu-gdpr:A13,
        eu-gdpr:A14,
        eu-gdpr:A15,
        eu-gdpr:A16,
        eu-gdpr:A17,
        eu-gdpr:A18,
        eu-gdpr:A20,
        eu-gdpr:A22,
        eu-gdpr:A7-3,
        eu-gdpr:A77 .

eu-gdpr:A6-1-a-explicit-consent a rdfs:Class,
        skos:Concept,
        dpv:LegalBasis ;
    dct:contributor _:N0a43dd9ea5e94fe695d8b7df8802cfdd,
        _:N2b1e6adbca7e4e73a4c12246fc8d2f06,
        _:N6bd5cc92354a4f6e91cef68caab7fcdd,
        _:Nd401626ea33444c4a84dfef86e49d9f5 ;
    dct:created "2022-06-22"^^xsd:date ;
    dct:modified "2024-12-17"^^xsd:date ;
    dct:source [ a schema:WebPage ;
            schema:name "GDPR Art.6-1a" ;
            schema:url "https://eur-lex.europa.eu/eli/reg/2016/679/art_6/par_1/pnt_a/oj" ] ;
    rdfs:isDefinedBy eu-gdpr: ;
    sw:term_status "accepted"@en ;
    skos:broader dpv:ExplicitlyExpressedConsent,
        eu-gdpr:A6-1-a,
        eu-gdpr:Consent ;
    skos:definition "Legal basis based on data subject's given explicit consent to the processing of his or her personal data for one or more specific purposes"@en ;
    skos:inScheme eu-gdpr:legal-basis-classes ;
    skos:prefLabel "Art 6(1-a) explicit consent"@en ;
    skos:scopeNote "Valid consent in this case would have requirements for being 'explicit' in addition to requirements defined by A4-11. This is also mentioned in the Article 29 Working Party document \"Guidelines on Consent under Regulation 2016/679 (wp259rev.01)\""@en ;
    dpv:hasRight eu-gdpr:A13,
        eu-gdpr:A14,
        eu-gdpr:A15,
        eu-gdpr:A16,
        eu-gdpr:A17,
        eu-gdpr:A18,
        eu-gdpr:A20,
        eu-gdpr:A22,
        eu-gdpr:A7-3,
        eu-gdpr:A77 .

eu-gdpr:A6-1-a-non-explicit-consent a rdfs:Class,
        skos:Concept,
        dpv:LegalBasis ;
    dct:contributor _:N0a43dd9ea5e94fe695d8b7df8802cfdd,
        _:N2b1e6adbca7e4e73a4c12246fc8d2f06,
        _:N6bd5cc92354a4f6e91cef68caab7fcdd,
        _:Nd401626ea33444c4a84dfef86e49d9f5 ;
    dct:created "2019-04-10"^^xsd:date ;
    dct:modified "2024-12-17"^^xsd:date ;
    dct:source [ a schema:WebPage ;
            schema:name "GDPR Art.6-1a" ;
            schema:url "https://eur-lex.europa.eu/eli/reg/2016/679/art_6/par_1/pnt_a/oj" ] ;
    rdfs:isDefinedBy eu-gdpr: ;
    sw:term_status "accepted"@en ;
    skos:broader dpv:ExpressedConsent,
        eu-gdpr:A6-1-a,
        eu-gdpr:Consent ;
    skos:definition "Legal basis based on data subject's given non-explicit express consent to the processing of his or her personal data for one or more specific purposes"@en ;
    skos:inScheme eu-gdpr:legal-basis-classes ;
    skos:prefLabel "Art.6(1-a) regular consent"@en ;
    skos:scopeNote "Definition of consent: A data subject's unambiguous/clear affirmative action that signifies an agreement to process their personal data (Rigo Wenning) . What is referred to as 'non-explicit consent' here is also termed as 'regular' consent in the Article 29 Working Party document \"Guidelines on Consent under Regulation 2016/679 (wp259rev.01)\". This is the legal basis that requires consent but not at the level of being 'explicit'."@en ;
    dpv:hasRight eu-gdpr:A13,
        eu-gdpr:A14,
        eu-gdpr:A15,
        eu-gdpr:A16,
        eu-gdpr:A17,
        eu-gdpr:A18,
        eu-gdpr:A20,
        eu-gdpr:A22,
        eu-gdpr:A7-3,
        eu-gdpr:A77 .

eu-gdpr:A6-1-b a rdfs:Class,
        skos:Concept,
        dpv:LegalBasis ;
    dct:contributor _:N0a43dd9ea5e94fe695d8b7df8802cfdd,
        _:N2b1e6adbca7e4e73a4c12246fc8d2f06,
        _:N6bd5cc92354a4f6e91cef68caab7fcdd ;
    dct:created "2019-04-05"^^xsd:date ;
    dct:modified "2022-11-24"^^xsd:date ;
    dct:source [ a schema:WebPage ;
            schema:name "GDPR Art.6-1b" ;
            schema:url "https://eur-lex.europa.eu/eli/reg/2016/679/art_6/par_1/pnt_b/oj" ] ;
    rdfs:isDefinedBy eu-gdpr: ;
    sw:term_status "accepted"@en ;
    skos:broader dpv:Contract ;
    skos:definition "Legal basis based on performance of a contract to which the data subject is party or in order to take steps at the request of the data subject prior to entering into a contract"@en ;
    skos:inScheme eu-gdpr:legal-basis-classes ;
    skos:prefLabel "Art 6(1-b) contract"@en ;
    dpv:hasRight eu-gdpr:A13,
        eu-gdpr:A14,
        eu-gdpr:A15,
        eu-gdpr:A16,
        eu-gdpr:A17,
        eu-gdpr:A18,
        eu-gdpr:A20,
        eu-gdpr:A22,
        eu-gdpr:A77 .

eu-gdpr:A6-1-b-contract-performance a rdfs:Class,
        skos:Concept,
        dpv:LegalBasis ;
    dct:contributor _:N05cd1f43dbaf4b4ba297dab5ee221394 ;
    dct:created "2022-11-24"^^xsd:date ;
    dct:modified "2022-11-24"^^xsd:date ;
    dct:source [ a schema:WebPage ;
            schema:name "GDPR Art.6-1b" ;
            schema:url "https://eur-lex.europa.eu/eli/reg/2016/679/art_6/par_1/pnt_b/oj" ] ;
    rdfs:isDefinedBy eu-gdpr: ;
    sw:term_status "accepted"@en ;
    skos:broader dpv:ContractPerformance,
        eu-gdpr:A6-1-b ;
    skos:definition "Legal basis based on performance of a contract to which the data subject is party"@en ;
    skos:inScheme eu-gdpr:legal-basis-classes ;
    skos:prefLabel "Art 6(1-b) contract performance"@en ;
    dpv:hasRight eu-gdpr:A13,
        eu-gdpr:A14,
        eu-gdpr:A15,
        eu-gdpr:A16,
        eu-gdpr:A17,
        eu-gdpr:A18,
        eu-gdpr:A20,
        eu-gdpr:A22,
        eu-gdpr:A77 .

eu-gdpr:A6-1-b-enter-into-contract a rdfs:Class,
        skos:Concept,
        dpv:LegalBasis ;
    dct:contributor _:N05cd1f43dbaf4b4ba297dab5ee221394 ;
    dct:created "2022-11-24"^^xsd:date ;
    dct:modified "2022-11-24"^^xsd:date ;
    dct:source [ a schema:WebPage ;
            schema:name "GDPR Art.6-1b" ;
            schema:url "https://eur-lex.europa.eu/eli/reg/2016/679/art_6/par_1/pnt_b/oj" ] ;
    rdfs:isDefinedBy eu-gdpr: ;
    sw:term_status "accepted"@en ;
    skos:broader dpv:EnterIntoContract,
        eu-gdpr:A6-1-b ;
    skos:definition "Legal basis based on taking steps at the request of the data subject prior to entering into a contract"@en ;
    skos:inScheme eu-gdpr:legal-basis-classes ;
    skos:prefLabel "Art 6(1-b) enter into contract"@en ;
    dpv:hasRight eu-gdpr:A13,
        eu-gdpr:A14,
        eu-gdpr:A15,
        eu-gdpr:A16,
        eu-gdpr:A17,
        eu-gdpr:A18,
        eu-gdpr:A20,
        eu-gdpr:A22,
        eu-gdpr:A77 .

eu-gdpr:A6-1-c a rdfs:Class,
        skos:Concept,
        dpv:LegalBasis ;
    dct:contributor _:N0a43dd9ea5e94fe695d8b7df8802cfdd,
        _:N2b1e6adbca7e4e73a4c12246fc8d2f06,
        _:N6bd5cc92354a4f6e91cef68caab7fcdd ;
    dct:created "2019-04-05"^^xsd:date ;
    dct:modified "2022-11-24"^^xsd:date ;
    dct:source [ a schema:WebPage ;
            schema:name "GDPR Art.6-1c" ;
            schema:url "https://eur-lex.europa.eu/eli/reg/2016/679/art_6/par_1/pnt_c/oj" ] ;
    rdfs:isDefinedBy eu-gdpr: ;
    sw:term_status "accepted"@en ;
    skos:broader dpv:LegalObligation ;
    skos:definition "Legal basis based on compliance with a legal obligation to which the controller is subject"@en ;
    skos:inScheme eu-gdpr:legal-basis-classes ;
    skos:prefLabel "Art 6(1-c) legal obligation"@en ;
    dpv:hasRight eu-gdpr:A13,
        eu-gdpr:A15,
        eu-gdpr:A16,
        eu-gdpr:A18,
        eu-gdpr:A77 .

eu-gdpr:A6-1-d a rdfs:Class,
        skos:Concept,
        dpv:LegalBasis ;
    dct:contributor _:N0a43dd9ea5e94fe695d8b7df8802cfdd,
        _:N2b1e6adbca7e4e73a4c12246fc8d2f06,
        _:N6bd5cc92354a4f6e91cef68caab7fcdd ;
    dct:created "2019-04-05"^^xsd:date ;
    dct:modified "2022-11-24"^^xsd:date ;
    dct:source [ a schema:WebPage ;
            schema:name "GDPR Art.6-1d" ;
            schema:url "https://eur-lex.europa.eu/eli/reg/2016/679/art_6/par_1/pnt_d/oj" ] ;
    rdfs:isDefinedBy eu-gdpr: ;
    sw:term_status "accepted"@en ;
    skos:broader dpv:VitalInterest ;
    skos:definition "Legal basis based on protecting the vital interests of the data subject or of another natural person"@en ;
    skos:inScheme eu-gdpr:legal-basis-classes ;
    skos:prefLabel "Art 6(1-d) protect vital interests"@en ;
    dpv:hasRight eu-gdpr:A13,
        eu-gdpr:A14,
        eu-gdpr:A15,
        eu-gdpr:A16,
        eu-gdpr:A17,
        eu-gdpr:A18,
        eu-gdpr:A22,
        eu-gdpr:A77 .

eu-gdpr:A6-1-d-data-subject a rdfs:Class,
        skos:Concept,
        dpv:LegalBasis ;
    dct:contributor _:N05cd1f43dbaf4b4ba297dab5ee221394 ;
    dct:created "2022-11-24"^^xsd:date ;
    dct:modified "2022-11-24"^^xsd:date ;
    dct:source [ a schema:WebPage ;
            schema:name "GDPR Art.6-1d" ;
            schema:url "https://eur-lex.europa.eu/eli/reg/2016/679/art_6/par_1/pnt_d/oj" ] ;
    rdfs:isDefinedBy eu-gdpr: ;
    sw:term_status "accepted"@en ;
    skos:broader dpv:VitalInterestOfDataSubject,
        eu-gdpr:A6-1-d ;
    skos:definition "Legal basis based on protecting the vital interests of the data subject"@en ;
    skos:inScheme eu-gdpr:legal-basis-classes ;
    skos:prefLabel "Art 6(1-d) protect vital interests of data subject"@en ;
    dpv:hasRight eu-gdpr:A13,
        eu-gdpr:A14,
        eu-gdpr:A15,
        eu-gdpr:A16,
        eu-gdpr:A17,
        eu-gdpr:A18,
        eu-gdpr:A22,
        eu-gdpr:A77 .

eu-gdpr:A6-1-d-natural-person a rdfs:Class,
        skos:Concept,
        dpv:LegalBasis ;
    dct:contributor _:N05cd1f43dbaf4b4ba297dab5ee221394 ;
    dct:created "2022-11-24"^^xsd:date ;
    dct:modified "2024-02-15"^^xsd:date ;
    dct:source [ a schema:WebPage ;
            schema:name "GDPR Art.6-1d" ;
            schema:url "https://eur-lex.europa.eu/eli/reg/2016/679/art_6/par_1/pnt_d/oj" ] ;
    rdfs:isDefinedBy eu-gdpr: ;
    sw:term_status "accepted"@en ;
    skos:broader dpv:VitalInterestOfNaturalPerson,
        eu-gdpr:A6-1-d ;
    skos:definition "Legal basis based on protecting the vital interests of another natural person that is not the data subject"@en ;
    skos:inScheme eu-gdpr:legal-basis-classes ;
    skos:prefLabel "Art 6(1-d) protect vital interests of natural person"@en .

eu-gdpr:A6-1-e a rdfs:Class,
        skos:Concept,
        dpv:LegalBasis ;
    dct:contributor _:N0a43dd9ea5e94fe695d8b7df8802cfdd,
        _:N2b1e6adbca7e4e73a4c12246fc8d2f06,
        _:N6bd5cc92354a4f6e91cef68caab7fcdd ;
    dct:created "2019-04-05"^^xsd:date ;
    dct:modified "2022-11-24"^^xsd:date ;
    dct:source [ a schema:WebPage ;
            schema:name "GDPR Art.6-1e" ;
            schema:url "https://eur-lex.europa.eu/eli/reg/2016/679/art_6/par_1/pnt_e/oj" ] ;
    rdfs:isDefinedBy eu-gdpr: ;
    sw:term_status "accepted"@en ;
    skos:broader dpv:OfficialAuthorityOfController,
        dpv:PublicInterest ;
    skos:definition "Legal basis based on performance of a task carried out in the public interest or in the exercise of official authority vested in the controller"@en ;
    skos:inScheme eu-gdpr:legal-basis-classes ;
    skos:prefLabel "Art 6(1-e) public interest or official authority"@en ;
    dpv:hasRight eu-gdpr:A13,
        eu-gdpr:A14,
        eu-gdpr:A15,
        eu-gdpr:A16,
        eu-gdpr:A18,
        eu-gdpr:A21,
        eu-gdpr:A22,
        eu-gdpr:A77 .

eu-gdpr:A6-1-e-official-authority a rdfs:Class,
        skos:Concept,
        dpv:LegalBasis ;
    dct:contributor _:N0a43dd9ea5e94fe695d8b7df8802cfdd ;
    dct:created "2022-08-24"^^xsd:date ;
    dct:modified "2022-11-24"^^xsd:date ;
    dct:source [ a schema:WebPage ;
            schema:name "GDPR Art.6-1e" ;
            schema:url "https://eur-lex.europa.eu/eli/reg/2016/679/art_6/par_1/pnt_e/oj" ] ;
    rdfs:isDefinedBy eu-gdpr: ;
    sw:term_status "accepted"@en ;
    skos:broader dpv:OfficialAuthorityOfController,
        eu-gdpr:A6-1-e ;
    skos:definition "Legal basis based on the exercise of official authority vested in the controller"@en ;
    skos:inScheme eu-gdpr:legal-basis-classes ;
    skos:prefLabel "Art 6(1-e) official authority"@en ;
    dpv:hasRight eu-gdpr:A13,
        eu-gdpr:A14,
        eu-gdpr:A15,
        eu-gdpr:A16,
        eu-gdpr:A18,
        eu-gdpr:A21,
        eu-gdpr:A22,
        eu-gdpr:A77 .

eu-gdpr:A6-1-e-public-interest a rdfs:Class,
        skos:Concept,
        dpv:LegalBasis ;
    dct:contributor _:N0a43dd9ea5e94fe695d8b7df8802cfdd ;
    dct:created "2022-08-24"^^xsd:date ;
    dct:modified "2022-11-24"^^xsd:date ;
    dct:source [ a schema:WebPage ;
            schema:name "GDPR Art.6-1e" ;
            schema:url "https://eur-lex.europa.eu/eli/reg/2016/679/art_6/par_1/pnt_e/oj" ] ;
    rdfs:isDefinedBy eu-gdpr: ;
    sw:term_status "accepted"@en ;
    skos:broader dpv:PublicInterest,
        eu-gdpr:A6-1-e ;
    skos:definition "Legal basis based on performance of a task carried out in the public interest"@en ;
    skos:inScheme eu-gdpr:legal-basis-classes ;
    skos:prefLabel "Art 6(1-e) public interest"@en ;
    dpv:hasRight eu-gdpr:A13,
        eu-gdpr:A14,
        eu-gdpr:A15,
        eu-gdpr:A16,
        eu-gdpr:A18,
        eu-gdpr:A21,
        eu-gdpr:A22,
        eu-gdpr:A77 .

eu-gdpr:A6-1-f a rdfs:Class,
        skos:Concept,
        dpv:LegalBasis ;
    dct:contributor _:N0a43dd9ea5e94fe695d8b7df8802cfdd,
        _:N2b1e6adbca7e4e73a4c12246fc8d2f06,
        _:N6bd5cc92354a4f6e91cef68caab7fcdd ;
    dct:created "2019-04-05"^^xsd:date ;
    dct:modified "2022-11-24"^^xsd:date ;
    dct:source [ a schema:WebPage ;
            schema:name "GDPR Art.6-1f" ;
            schema:url "https://eur-lex.europa.eu/eli/reg/2016/679/art_6/par_1/pnt_f/oj" ] ;
    rdfs:isDefinedBy eu-gdpr: ;
    sw:term_status "accepted"@en ;
    skos:broader dpv:LegitimateInterest ;
    skos:definition "Legal basis based on the purposes of the legitimate interests pursued by the controller or by a third party, except where such interests are overridden by the interests or fundamental rights and freedoms of the data subject which require protection of personal data, in particular where the data subject is a child"@en ;
    skos:inScheme eu-gdpr:legal-basis-classes ;
    skos:prefLabel "Art 6(1-f) legitimate interest"@en ;
    dpv:hasRight eu-gdpr:A13,
        eu-gdpr:A14,
        eu-gdpr:A15,
        eu-gdpr:A16,
        eu-gdpr:A17,
        eu-gdpr:A18,
        eu-gdpr:A21,
        eu-gdpr:A22,
        eu-gdpr:A77 .

eu-gdpr:A6-1-f-controller a rdfs:Class,
        skos:Concept,
        dpv:LegalBasis ;
    dct:contributor _:N05cd1f43dbaf4b4ba297dab5ee221394 ;
    dct:created "2022-11-24"^^xsd:date ;
    dct:modified "2022-11-24"^^xsd:date ;
    dct:source [ a schema:WebPage ;
            schema:name "GDPR Art.6-1f" ;
            schema:url "https://eur-lex.europa.eu/eli/reg/2016/679/art_6/par_1/pnt_f/oj" ] ;
    rdfs:isDefinedBy eu-gdpr: ;
    sw:term_status "accepted"@en ;
    skos:broader dpv:LegitimateInterestOfController,
        eu-gdpr:A6-1-f ;
    skos:definition "Legal basis based on the purposes of the legitimate interests pursued by the controller, except where such interests are overridden by the interests or fundamental rights and freedoms of the data subject which require protection of personal data, in particular where the data subject is a child"@en ;
    skos:inScheme eu-gdpr:legal-basis-classes ;
    skos:prefLabel "Art 6(1-f) legitimate interest of controller"@en ;
    dpv:hasRight eu-gdpr:A13,
        eu-gdpr:A14,
        eu-gdpr:A15,
        eu-gdpr:A16,
        eu-gdpr:A17,
        eu-gdpr:A18,
        eu-gdpr:A21,
        eu-gdpr:A22,
        eu-gdpr:A77 .

eu-gdpr:A6-1-f-third-party a rdfs:Class,
        skos:Concept,
        dpv:LegalBasis ;
    dct:contributor _:N05cd1f43dbaf4b4ba297dab5ee221394 ;
    dct:created "2022-11-24"^^xsd:date ;
    dct:modified "2022-11-24"^^xsd:date ;
    dct:source [ a schema:WebPage ;
            schema:name "GDPR Art.6-1f" ;
            schema:url "https://eur-lex.europa.eu/eli/reg/2016/679/art_6/par_1/pnt_f/oj" ] ;
    rdfs:isDefinedBy eu-gdpr: ;
    sw:term_status "accepted"@en ;
    skos:broader dpv:LegitimateInterestOfThirdParty,
        eu-gdpr:A6-1-f ;
    skos:definition "Legal basis based on the purposes of the legitimate interests pursued by a third party, except where such interests are overridden by the interests or fundamental rights and freedoms of the data subject which require protection of personal data, in particular where the data subject is a child"@en ;
    skos:inScheme eu-gdpr:legal-basis-classes ;
    skos:prefLabel "Art 6(1-f) legitimate interest of third party"@en ;
    dpv:hasRight eu-gdpr:A13,
        eu-gdpr:A14,
        eu-gdpr:A15,
        eu-gdpr:A16,
        eu-gdpr:A17,
        eu-gdpr:A18,
        eu-gdpr:A21,
        eu-gdpr:A22,
        eu-gdpr:A77 .

eu-gdpr:A7-3 a rdfs:Class,
        skos:Concept,
        dpv:Right ;
    dct:contributor _:N05cd1f43dbaf4b4ba297dab5ee221394,
        _:N0a43dd9ea5e94fe695d8b7df8802cfdd,
        _:N458008bc6195484e9cc557f70eabda31 ;
    dct:created "2020-11-04"^^xsd:date ;
    dct:source [ a schema:WebPage ;
            schema:name "GDPR Art.7-3" ;
            schema:url "https://eur-lex.europa.eu/eli/reg/2016/679/art_7/par_3/oj" ] ;
    rdfs:isDefinedBy eu-gdpr: ;
    sw:term_status "accepted"@en ;
    skos:broader dpv:DataSubjectRight ;
    skos:definition "Right to withdraw consent at any time"@en ;
    skos:inScheme eu-gdpr:rights-classes ;
    skos:prefLabel "A7-3 Right to Withdraw Consent"@en .

eu-gdpr:A7-3-Impact a rdfs:Class,
        skos:Concept,
        risk:PotentialConsequence,
        risk:PotentialImpact,
        risk:PotentialRisk,
        risk:RiskConcept ;
    dct:created "2024-10-21"^^xsd:date ;
    dct:source [ a schema:WebPage ;
            schema:name "GDPR Art.7-3" ;
            schema:url "https://eur-lex.europa.eu/eli/reg/2016/679/art_7/par_3/oj" ] ;
    rdfs:isDefinedBy eu-gdpr: ;
    sw:term_status "accepted"@en ;
    skos:broader eu-gdpr:GDPRRightsImpact ;
    skos:definition "Something that acts as or is considered as an impact on A7-3 Right to Withdraw Consent"@en ;
    skos:inScheme eu-gdpr:rights-impacts-classes ;
    skos:prefLabel "Impact on A7-3 Right to Withdraw Consent"@en .

eu-gdpr:A77 a rdfs:Class,
        skos:Concept,
        dpv:Right ;
    dct:contributor _:N05cd1f43dbaf4b4ba297dab5ee221394,
        _:N0a43dd9ea5e94fe695d8b7df8802cfdd,
        _:N458008bc6195484e9cc557f70eabda31 ;
    dct:created "2020-11-04"^^xsd:date ;
    dct:source [ a schema:WebPage ;
            schema:name "GDPR Art.77" ;
            schema:url "https://eur-lex.europa.eu/eli/reg/2016/679/art_77/oj" ] ;
    rdfs:isDefinedBy eu-gdpr: ;
    sw:term_status "accepted"@en ;
    skos:broader dpv:DataSubjectRight ;
    skos:definition "Right to lodge a complaint with a supervisory authority"@en ;
    skos:inScheme eu-gdpr:rights-classes ;
    skos:prefLabel "A77 Right to Complaint"@en .

eu-gdpr:A77-Impact a rdfs:Class,
        skos:Concept,
        risk:PotentialConsequence,
        risk:PotentialImpact,
        risk:PotentialRisk,
        risk:RiskConcept ;
    dct:created "2024-10-21"^^xsd:date ;
    dct:source [ a schema:WebPage ;
            schema:name "GDPR Art.77" ;
            schema:url "https://eur-lex.europa.eu/eli/reg/2016/679/art_77/oj" ] ;
    rdfs:isDefinedBy eu-gdpr: ;
    sw:term_status "accepted"@en ;
    skos:broader eu-gdpr:GDPRRightsImpact ;
    skos:definition "Something that acts as or is considered as an impact on A77 Right to Complaint"@en ;
    skos:inScheme eu-gdpr:rights-impacts-classes ;
    skos:prefLabel "Impact on A77 Right to Complaint"@en .

eu-gdpr:A78 a rdfs:Class,
        skos:Concept,
        dpv:Right ;
    dct:contributor _:N05cd1f43dbaf4b4ba297dab5ee221394,
        _:N0a43dd9ea5e94fe695d8b7df8802cfdd,
        _:N458008bc6195484e9cc557f70eabda31 ;
    dct:created "2024-12-17"^^xsd:date ;
    dct:source [ a schema:WebPage ;
            schema:name "GDPR Art.78" ;
            schema:url "https://eur-lex.europa.eu/eli/reg/2016/679/art_78/oj" ] ;
    rdfs:isDefinedBy eu-gdpr: ;
    sw:term_status "accepted"@en ;
    skos:broader dpv:Right ;
    skos:definition "Right to an effective judicial remedy against a legally binding decision of a supervisory authority concerning natural or legal person"@en ;
    skos:inScheme eu-gdpr:rights-classes ;
    skos:prefLabel "A78 Right to an effective judicial remedy against a supervisory authority"@en .

eu-gdpr:A79 a rdfs:Class,
        skos:Concept,
        dpv:Right ;
    dct:contributor _:N05cd1f43dbaf4b4ba297dab5ee221394,
        _:N0a43dd9ea5e94fe695d8b7df8802cfdd,
        _:N458008bc6195484e9cc557f70eabda31 ;
    dct:created "2024-12-17"^^xsd:date ;
    dct:source [ a schema:WebPage ;
            schema:name "GDPR Art.79" ;
            schema:url "https://eur-lex.europa.eu/eli/reg/2016/679/art_79/oj" ] ;
    rdfs:isDefinedBy eu-gdpr: ;
    sw:term_status "accepted"@en ;
    skos:broader dpv:DataSubjectRight ;
    skos:definition "Right to an effective judicial remedy where the data subject considers that his or her rights have been infringed as a result of the processing of his or her personal data"@en ;
    skos:inScheme eu-gdpr:rights-classes ;
    skos:prefLabel "A79 Right to an effective judicial remedy against a controller or processor"@en .

eu-gdpr:A9-2-a a rdfs:Class,
        skos:Concept,
        dpv:LegalBasis ;
    dct:contributor _:N2b1e6adbca7e4e73a4c12246fc8d2f06,
        _:N6bd5cc92354a4f6e91cef68caab7fcdd ;
    dct:created "2019-04-05"^^xsd:date ;
    dct:modified "2024-12-17"^^xsd:date ;
    dct:source [ a schema:WebPage ;
            schema:name "GDPR Art.9-2a" ;
            schema:url "https://eur-lex.europa.eu/eli/reg/2016/679/art_9/par_2/pnt_a/oj" ] ;
    rdfs:isDefinedBy eu-gdpr: ;
    sw:term_status "modified"@en ;
    skos:broader dpv:ExplicitlyExpressedConsent,
        eu-gdpr:Consent ;
    skos:definition "explicit consent with special categories of data"@en ;
    skos:inScheme eu-gdpr:legal-basis-special-classes ;
    skos:prefLabel "Art 9(2-a) explicit consent"@en .

eu-gdpr:A9-2-b a rdfs:Class,
        skos:Concept,
        dpv:LegalBasis ;
    dct:contributor _:N2b1e6adbca7e4e73a4c12246fc8d2f06,
        _:N6bd5cc92354a4f6e91cef68caab7fcdd ;
    dct:created "2019-04-05"^^xsd:date ;
    dct:source [ a schema:WebPage ;
            schema:name "GDPR Art.9-2b" ;
            schema:url "https://eur-lex.europa.eu/eli/reg/2016/679/art_9/par_2/pnt_b/oj" ] ;
    rdfs:isDefinedBy eu-gdpr: ;
    sw:term_status "accepted"@en ;
    skos:broader dpv:LegalBasis ;
    skos:definition "employment and social security and social protection law"@en ;
    skos:inScheme eu-gdpr:legal-basis-special-classes ;
    skos:prefLabel "Art 9(2-b) employment, social security, social protection law"@en .

eu-gdpr:A9-2-c a rdfs:Class,
        skos:Concept,
        dpv:LegalBasis ;
    dct:contributor _:N2b1e6adbca7e4e73a4c12246fc8d2f06,
        _:N6bd5cc92354a4f6e91cef68caab7fcdd ;
    dct:created "2019-04-05"^^xsd:date ;
    dct:modified "2021-09-08"^^xsd:date ;
    dct:source [ a schema:WebPage ;
            schema:name "GDPR Art.9-2c" ;
            schema:url "https://eur-lex.europa.eu/eli/reg/2016/679/art_9/par_2/pnt_c/oj" ] ;
    rdfs:isDefinedBy eu-gdpr: ;
    sw:term_status "accepted"@en ;
    skos:broader dpv:VitalInterest ;
    skos:definition "protection of the vital interests"@en ;
    skos:inScheme eu-gdpr:legal-basis-special-classes ;
    skos:prefLabel "Art 9(2-c) protect vital interest"@en .

eu-gdpr:A9-2-d a rdfs:Class,
        skos:Concept,
        dpv:LegalBasis ;
    dct:contributor _:N2b1e6adbca7e4e73a4c12246fc8d2f06,
        _:N6bd5cc92354a4f6e91cef68caab7fcdd ;
    dct:created "2019-04-05"^^xsd:date ;
    dct:modified "2021-09-08"^^xsd:date ;
    dct:source [ a schema:WebPage ;
            schema:name "GDPR Art.9-2d" ;
            schema:url "https://eur-lex.europa.eu/eli/reg/2016/679/art_9/par_2/pnt_d/oj" ] ;
    rdfs:isDefinedBy eu-gdpr: ;
    sw:term_status "accepted"@en ;
    skos:broader dpv:LegitimateInterest ;
    skos:definition "legitimate activities with appropriate safeguards by a foundation, association or any other not-for-profit body with a political, philosophical, religious or trade union aim and on condition that the processing relates solely to the members or to former members of the body or to persons who have regular contact with it in connection with its purposes and that the personal data are not disclosed outside that body without the consent of the data subjects;"@en ;
    skos:inScheme eu-gdpr:legal-basis-special-classes ;
    skos:prefLabel "Art 9(2-d) legitimate activities"@en .

eu-gdpr:A9-2-e a rdfs:Class,
        skos:Concept,
        dpv:LegalBasis ;
    dct:contributor _:N2b1e6adbca7e4e73a4c12246fc8d2f06,
        _:N6bd5cc92354a4f6e91cef68caab7fcdd ;
    dct:created "2019-04-05"^^xsd:date ;
    dct:source [ a schema:WebPage ;
            schema:name "GDPR Art.9-2e" ;
            schema:url "https://eur-lex.europa.eu/eli/reg/2016/679/art_9/par_2/pnt_e/oj" ] ;
    rdfs:isDefinedBy eu-gdpr: ;
    sw:term_status "accepted"@en ;
    skos:broader dpv:LegalBasis ;
    skos:definition "data manifestly made public by the data subject"@en ;
    skos:inScheme eu-gdpr:legal-basis-special-classes ;
    skos:prefLabel "Art 9(2-e) data made public"@en .

eu-gdpr:A9-2-f a rdfs:Class,
        skos:Concept,
        dpv:LegalBasis ;
    dct:contributor _:N2b1e6adbca7e4e73a4c12246fc8d2f06,
        _:N6bd5cc92354a4f6e91cef68caab7fcdd ;
    dct:created "2019-04-05"^^xsd:date ;
    dct:source [ a schema:WebPage ;
            schema:name "GDPR Art.9-2f" ;
            schema:url "https://eur-lex.europa.eu/eli/reg/2016/679/art_9/par_2/pnt_f/oj" ] ;
    rdfs:isDefinedBy eu-gdpr: ;
    sw:term_status "accepted"@en ;
    skos:broader dpv:LegalBasis ;
    skos:definition "establishment, exercise or defence of legal claims / courts acting in their judicial capacity"@en ;
    skos:inScheme eu-gdpr:legal-basis-special-classes ;
    skos:prefLabel "Art 9(2-f) judicial process"@en .

eu-gdpr:A9-2-g a rdfs:Class,
        skos:Concept,
        dpv:LegalBasis ;
    dct:contributor _:N2b1e6adbca7e4e73a4c12246fc8d2f06,
        _:N6bd5cc92354a4f6e91cef68caab7fcdd ;
    dct:created "2019-04-05"^^xsd:date ;
    dct:modified "2021-09-08"^^xsd:date ;
    dct:source [ a schema:WebPage ;
            schema:name "GDPR Art.9-2g" ;
            schema:url "https://eur-lex.europa.eu/eli/reg/2016/679/art_9/par_2/pnt_g/oj" ] ;
    rdfs:isDefinedBy eu-gdpr: ;
    sw:term_status "accepted"@en ;
    skos:broader dpv:PublicInterest ;
    skos:definition "substantial public interest, on the basis of Union or Member State law"@en ;
    skos:inScheme eu-gdpr:legal-basis-special-classes ;
    skos:prefLabel "Art 9(2-g) public interest"@en .

eu-gdpr:A9-2-h a rdfs:Class,
        skos:Concept,
        dpv:LegalBasis ;
    dct:contributor _:N2b1e6adbca7e4e73a4c12246fc8d2f06,
        _:N6bd5cc92354a4f6e91cef68caab7fcdd ;
    dct:created "2019-04-05"^^xsd:date ;
    dct:source [ a schema:WebPage ;
            schema:name "GDPR Art.9-2h" ;
            schema:url "https://eur-lex.europa.eu/eli/reg/2016/679/art_9/par_2/pnt_h/oj" ] ;
    rdfs:isDefinedBy eu-gdpr: ;
    sw:term_status "accepted"@en ;
    skos:broader dpv:LegalBasis ;
    skos:definition "preventive or occupational medicine, for the assessment of the working capacity of the employee, medical diagnosis, the provision of health or social care or treatment or the management of health or social care systems and services on the basis of Union or Member State law or pursuant to contract with a health professional and subject to the conditions and safeguards referred to in paragraph 3"@en ;
    skos:inScheme eu-gdpr:legal-basis-special-classes ;
    skos:prefLabel "Art 9(2-h) health & medicine"@en .

eu-gdpr:A9-2-i a rdfs:Class,
        skos:Concept,
        dpv:LegalBasis ;
    dct:contributor _:N2b1e6adbca7e4e73a4c12246fc8d2f06,
        _:N6bd5cc92354a4f6e91cef68caab7fcdd ;
    dct:created "2019-04-05"^^xsd:date ;
    dct:modified "2021-09-08"^^xsd:date ;
    dct:source [ a schema:WebPage ;
            schema:name "GDPR Art.9-2i" ;
            schema:url "https://eur-lex.europa.eu/eli/reg/2016/679/art_9/par_2/pnt_i/oj" ] ;
    rdfs:isDefinedBy eu-gdpr: ;
    sw:term_status "accepted"@en ;
    skos:broader dpv:PublicInterest ;
    skos:definition "public interest in public health"@en ;
    skos:inScheme eu-gdpr:legal-basis-special-classes ;
    skos:prefLabel "Art 9(2-i) public interest in public health"@en .

eu-gdpr:A9-2-j a rdfs:Class,
        skos:Concept,
        dpv:LegalBasis ;
    dct:contributor _:N2b1e6adbca7e4e73a4c12246fc8d2f06,
        _:N6bd5cc92354a4f6e91cef68caab7fcdd ;
    dct:created "2019-04-05"^^xsd:date ;
    dct:modified "2021-09-08"^^xsd:date ;
    dct:source [ a schema:WebPage ;
            schema:name "GDPR Art.9-2j" ;
            schema:url "https://eur-lex.europa.eu/eli/reg/2016/679/art_9/par_2/pnt_j/oj" ] ;
    rdfs:isDefinedBy eu-gdpr: ;
    sw:term_status "accepted"@en ;
    skos:broader dpv:PublicInterest ;
    skos:definition "public interest, scientific or historical research purposes or statistical purposes based on Union or Member State law"@en ;
    skos:inScheme eu-gdpr:legal-basis-special-classes ;
    skos:prefLabel "Art 9(2-j) public interest, scientific research, statistical purpose"@en .

eu-gdpr:AccountabilityPrinciple a rdfs:Class,
        skos:Concept,
        dpv:OrganisationalMeasure ;
    dct:contributor _:N05cd1f43dbaf4b4ba297dab5ee221394 ;
    dct:created "2024-05-12"^^xsd:date ;
    dct:source "GDPR Art.5-2"@en ;
    rdfs:isDefinedBy eu-gdpr: ;
    sw:term_status "accepted"@en ;
    skos:broader dpv:Principle ;
    skos:definition "Principle stating the controller shall be responsible for, and be able to demonstrate compliance with the other principles (from Art.5-1)"@en ;
    skos:inScheme eu-gdpr:principles-classes ;
    skos:prefLabel "Accountability Principle"@en .

eu-gdpr:AccuracyPrinciple a rdfs:Class,
        skos:Concept,
        dpv:OrganisationalMeasure ;
    dct:contributor _:N05cd1f43dbaf4b4ba297dab5ee221394 ;
    dct:created "2024-05-12"^^xsd:date ;
    dct:source "GDPR Art.5-1d"@en ;
    rdfs:isDefinedBy eu-gdpr: ;
    sw:term_status "accepted"@en ;
    skos:broader dpv:Principle ;
    skos:definition "Principle stating personal data must be accurate and, where necessary, kept up to date; every reasonable step must be taken to ensure that personal data that are inaccurate, having regard to the purposes for which they are processed, are erased or rectified without delay used for"@en ;
    skos:inScheme eu-gdpr:principles-classes ;
    skos:prefLabel "Accuracy Principle"@en .

eu-gdpr:AdHocContractualClauses a rdfs:Class,
        skos:Concept,
        dpv:OrganisationalMeasure ;
    dct:contributor _:N0a43dd9ea5e94fe695d8b7df8802cfdd ;
    dct:created "2021-09-22"^^xsd:date ;
    dct:source [ a schema:WebPage ;
            schema:name "EDPB Recommendations 01/2020 on Supplementary Measures and Transfer Tools" ;
            schema:url "https://edpb.europa.eu/system/files/2021-06/edpb_recommendations_202001vo.2.0_supplementarymeasurestransferstools_en.pdf" ] ;
    rdfs:isDefinedBy eu-gdpr: ;
    sw:term_status "accepted"@en ;
    skos:broader dpv:Contract,
        eu-gdpr:DataTransferTool ;
    skos:definition "Contractual Clauses not drafted by the EU Commission, e.g. by the Controller"@en ;
    skos:inScheme eu-gdpr:data-transfers-classes ;
    skos:prefLabel "AdHoc Contractual Clauses"@en .

eu-gdpr:AdequacyDecision a rdfs:Class,
        skos:Concept,
        dpv:LegalBasis ;
    dct:contributor _:N0a43dd9ea5e94fe695d8b7df8802cfdd ;
    dct:created "2024-06-22"^^xsd:date ;
    dct:source [ a schema:WebPage ;
            schema:name "GDPR Art.45-3" ;
            schema:url "https://eur-lex.europa.eu/eli/reg/2016/679/art_45/par_3/oj" ] ;
    rdfs:isDefinedBy eu-gdpr: ;
    sw:term_status "accepted"@en ;
    skos:broader eu-gdpr:A45-3 ;
    skos:definition "An adequacy decision as per GDPR Art.45(3) for the transfer of data to a third country or an international organisation"@en ;
    skos:inScheme eu-gdpr:legal-basis-data-transfer-classes ;
    skos:prefLabel "Adequacy Decision"@en .

eu-gdpr:AvailabilityBreach a rdfs:Class,
        skos:Concept ;
    dct:created "2024-05-19"^^xsd:date ;
    dct:source "EDPB Guidelines 9/2022 on personal data breach notification under GDPR"@en ;
    rdfs:isDefinedBy eu-gdpr: ;
    rdfs:subClassOf eu-gdpr:DataBreach ;
    sw:term_status "accepted"@en ;
    skos:broader eu-gdpr:DataBreach ;
    skos:definition "A data breach where there is an accidental or unauthorised loss of access to or destruction of personal data"@en ;
    skos:inScheme eu-gdpr:data-breach-classes ;
    skos:prefLabel "Availability Breach"@en .

eu-gdpr:BindingCorporateRules a rdfs:Class,
        skos:Concept,
        dpv:OrganisationalMeasure ;
    dct:contributor _:N05cd1f43dbaf4b4ba297dab5ee221394,
        _:N0a43dd9ea5e94fe695d8b7df8802cfdd,
        _:N1aa8f48a4f3a40e6a438f71be918d3a1,
        _:Nd0960ac69a57403fb5db2455be10d160 ;
    dct:created "2021-09-22"^^xsd:date ;
    dct:source [ a schema:WebPage ;
            schema:name "GDPR Art.4-20" ;
            schema:url "https://eur-lex.europa.eu/eli/reg/2016/679/art_4/par_20/oj" ] ;
    rdfs:isDefinedBy eu-gdpr: ;
    sw:term_status "accepted"@en ;
    skos:broader eu-gdpr:DataTransferTool ;
    skos:definition "‘Binding Corporate Rules’ means personal data protection policies which are adhered to by a controller or processor established on the territory of a Member State for transfers or a set of transfers of personal data to a controller or processor in one or more third countries within a group of undertakings, or group of enterprises engaged in a joint economic activity"@en ;
    skos:inScheme eu-gdpr:data-transfers-classes ;
    skos:prefLabel "Binding Corporate Rules (BCR)"@en ;
    skos:scopeNote "Binding corporate rules (BCR) are data protection policies adhered to by companies established in the EU for transfers of personal data outside the EU within a group of undertakings or enterprises."@en .

eu-gdpr:BiometricData a rdfs:Class,
        skos:Concept,
        pd:Biometric ;
    dct:contributor _:N0a43dd9ea5e94fe695d8b7df8802cfdd ;
    dct:created "2024-12-17"^^xsd:date ;
    rdf:value "dpv:PersonalData" ;
    rdfs:isDefinedBy eu-gdpr: ;
    sw:term_status "accepted"@en ;
    skos:broader pd:Biometric ;
    skos:definition "‘Biometric Data’ means personal data resulting from specific technical processing relating to the physical, physiological or behavioural characteristics of a natural person, which allow or confirm the unique identification of that natural person, such as facial images or dactyloscopic data"@en ;
    skos:inScheme eu-gdpr:misc-concepts-classes ;
    skos:prefLabel "Biometric Data"@en .

eu-gdpr:BreachNotificationNotNeeded a rdfs:Class,
        skos:Concept,
        eu-gdpr:DataBreachNoticeRequirement ;
    dct:created "2024-05-19"^^xsd:date ;
    dct:source "GDPR Article 33"@en ;
    rdfs:isDefinedBy eu-gdpr: ;
    sw:term_status "accepted"@en ;
    skos:broader eu-gdpr:DataBreachNoticeRequirement ;
    skos:definition "Data Breach notifications to DPA or Data Subjects are not required"@en ;
    skos:inScheme eu-gdpr:data-breach-classes ;
    skos:prefLabel "Breach Notification Not Needed"@en .

eu-gdpr:CertificationMechanismsForDataTransfers a rdfs:Class,
        skos:Concept,
        dpv:OrganisationalMeasure ;
    dct:contributor _:N0a43dd9ea5e94fe695d8b7df8802cfdd ;
    dct:created "2021-09-22"^^xsd:date ;
    dct:source [ a schema:WebPage ;
            schema:name "EDPB Recommendations 01/2020 on Supplementary Measures and Transfer Tools" ;
            schema:url "https://edpb.europa.eu/system/files/2021-06/edpb_recommendations_202001vo.2.0_supplementarymeasurestransferstools_en.pdf" ] ;
    rdfs:isDefinedBy eu-gdpr: ;
    sw:term_status "accepted"@en ;
    skos:broader eu-gdpr:DataTransferTool ;
    skos:definition "Certification and its binding or specified mechanisms intended to provide sufficient safeguards for data transfers"@en ;
    skos:inScheme eu-gdpr:data-transfers-classes ;
    skos:prefLabel "Certification Mechanisms for Data Transfers"@en .

eu-gdpr:CodesOfConductForDataTransfers a rdfs:Class,
        skos:Concept,
        dpv:OrganisationalMeasure ;
    dct:contributor _:N0a43dd9ea5e94fe695d8b7df8802cfdd ;
    dct:created "2021-09-22"^^xsd:date ;
    dct:source [ a schema:WebPage ;
            schema:name "EDPB Recommendations 01/2020 on Supplementary Measures and Transfer Tools" ;
            schema:url "https://edpb.europa.eu/system/files/2021-06/edpb_recommendations_202001vo.2.0_supplementarymeasurestransferstools_en.pdf" ] ;
    rdfs:isDefinedBy eu-gdpr: ;
    sw:term_status "accepted"@en ;
    skos:broader eu-gdpr:DataTransferTool ;
    skos:definition "Codes of Conduct that outline sufficient safeguards for carrying out data transfers"@en ;
    skos:inScheme eu-gdpr:data-transfers-classes ;
    skos:prefLabel "Codes of Conduct for Data Transfers"@en .

eu-gdpr:ConcernedSupervisoryAuthority a rdfs:Class,
        skos:Concept ;
    dct:contributor _:N05cd1f43dbaf4b4ba297dab5ee221394,
        _:N0a43dd9ea5e94fe695d8b7df8802cfdd ;
    dct:created "2024-02-14"^^xsd:date ;
    dct:source " Guidelines 3/2018 on the territorial scope of the GDPR (Article 3) Version 2.1"@en,
        "GDPR Art.56"@en ;
    rdfs:isDefinedBy eu-gdpr: ;
    rdfs:subClassOf eu-gdpr:DataProtectionAuthority ;
    sw:term_status "accepted"@en ;
    skos:broader eu-gdpr:DataProtectionAuthority ;
    skos:definition "Concerned Supervisory Authority' or 'supervisory authority concerned’ means a supervisory authority which is concerned by the processing of personal data because: (a) the controller or processor is established on the territory of the Member State of that supervisory authority; (b) data subjects residing in the Member State of that supervisory authority are substantially affected or likely to be substantially affected by the processing; or (c) a complaint has been lodged with that supervisory authority"@en ;
    skos:inScheme eu-gdpr:entities-classes ;
    skos:prefLabel "Concerned Supervisory Authority"@en .

eu-gdpr:ConfidentialityBreach a rdfs:Class,
        skos:Concept ;
    dct:created "2024-05-19"^^xsd:date ;
    dct:source "EDPB Guidelines 9/2022 on personal data breach notification under GDPR"@en ;
    rdfs:isDefinedBy eu-gdpr: ;
    rdfs:subClassOf eu-gdpr:DataBreach ;
    sw:term_status "accepted"@en ;
    skos:broader eu-gdpr:DataBreach ;
    skos:definition "A data breach where there is an unauthorised or accidental disclosure of or access to personal data"@en ;
    skos:inScheme eu-gdpr:data-breach-classes ;
    skos:prefLabel "Confidentiality Breach"@en .

eu-gdpr:Consent a rdfs:Class,
        skos:Concept,
        dpv:LegalBasis ;
    dct:contributor _:N0a43dd9ea5e94fe695d8b7df8802cfdd ;
    dct:created "2024-12-17"^^xsd:date ;
    dct:source [ a schema:WebPage ;
            schema:name "GDPR Art.4-11" ;
            schema:url "https://eur-lex.europa.eu/eli/reg/2016/679/art_4/par_11/oj" ] ;
    rdfs:isDefinedBy eu-gdpr: ;
    sw:term_status "accepted"@en ;
    skos:broader dpv:Consent ;
    skos:definition "Consent’ of the data subject means any freely given, specific, informed and unambiguous indication of the data subject’s wishes by which he or she, by a statement or by a clear affirmative action, signifies agreement to the processing of personal data relating to him or her"@en ;
    skos:inScheme eu-gdpr:legal-basis-classes ;
    skos:prefLabel "Consent"@en .

eu-gdpr:Controller a rdfs:Class,
        skos:Concept ;
    dct:contributor _:N0a43dd9ea5e94fe695d8b7df8802cfdd ;
    dct:created "2024-12-17"^^xsd:date ;
    dct:source "GDPR Art.4-7"@en ;
    rdfs:isDefinedBy eu-gdpr: ;
    rdfs:subClassOf dpv:DataController ;
    sw:term_status "accepted"@en ;
    skos:broader dpv:DataController ;
    skos:definition "‘Controller’ means the natural or legal person, public authority, agency or other body which, alone or jointly with others, determines the purposes and means of the processing of personal data; where the purposes and means of such processing are determined by Union or Member State law, the controller or the specific criteria for its nomination may be provided for by Union or Member State law"@en ;
    skos:inScheme eu-gdpr:entities-classes ;
    skos:prefLabel "Controller"@en .

eu-gdpr:ControllerBreachNotice a rdfs:Class,
        skos:Concept,
        eu-gdpr:DataBreachNotice ;
    dct:created "2024-05-19"^^xsd:date ;
    dct:source "GDPR Article 33"@en ;
    rdfs:isDefinedBy eu-gdpr: ;
    sw:term_status "accepted"@en ;
    skos:broader eu-gdpr:DataBreachNotice ;
    skos:definition "Notice regarding a data breach to the Controller"@en ;
    skos:inScheme eu-gdpr:data-breach-classes ;
    skos:prefLabel "Controller Breach Notice"@en .

eu-gdpr:ControllerBreachNotificationNeeded a rdfs:Class,
        skos:Concept,
        eu-gdpr:DataBreachNoticeRequirement ;
    dct:created "2024-05-19"^^xsd:date ;
    dct:source "GDPR Article 33"@en ;
    rdfs:isDefinedBy eu-gdpr: ;
    sw:term_status "accepted"@en ;
    skos:broader eu-gdpr:DataBreachNoticeRequirement ;
    skos:definition "Data Breach notification to the Controller is required"@en ;
    skos:inScheme eu-gdpr:data-breach-classes ;
    skos:prefLabel "Controller Breach Notification Needed"@en .

eu-gdpr:CrossBorderDataBreach a rdfs:Class,
        skos:Concept ;
    dct:created "2024-05-19"^^xsd:date ;
    dct:source "EDPB Guidelines 9/2022 on personal data breach notification under GDPR"@en ;
    rdfs:isDefinedBy eu-gdpr: ;
    rdfs:subClassOf eu-gdpr:DataBreach ;
    sw:term_status "accepted"@en ;
    skos:broader eu-gdpr:DataBreach ;
    skos:definition "A data breach involving cross-border data subjects or processing operations"@en ;
    skos:inScheme eu-gdpr:data-breach-classes ;
    skos:prefLabel "Cross-Border Data Breach"@en .

eu-gdpr:CrossBorderProcessing a rdfs:Class,
        skos:Concept,
        dpv:Processing ;
    dct:contributor _:N0a43dd9ea5e94fe695d8b7df8802cfdd ;
    dct:created "2024-12-17"^^xsd:date ;
    rdf:value "sc" ;
    rdfs:isDefinedBy eu-gdpr: ;
    sw:term_status "accepted"@en ;
    skos:broader dpv:Processing ;
    skos:definition "‘Cross-Border Processing’ means either: (a) processing of personal data which takes place in the context of the activities of establishments in more than one Member State of a controller or processor in the Union where the controller or processor is established in more than one Member State; or (b)  processing of personal data which takes place in the context of the activities of a single establishment of a controller or processor in the Union but which substantially affects or is likely to substantially affect data subjects in more than one Member State"@en ;
    skos:inScheme eu-gdpr:misc-concepts-classes ;
    skos:prefLabel "Cross Border Processing"@en .

eu-gdpr:DBIAIndicatesHighRisk a rdfs:Class,
        skos:Concept,
        eu-gdpr:DBIARiskStatus ;
    dct:contributor _:N0a43dd9ea5e94fe695d8b7df8802cfdd ;
    dct:created "2024-05-19"^^xsd:date ;
    dct:source "GDPR Article 33"@en ;
    rdfs:isDefinedBy eu-gdpr: ;
    sw:term_status "accepted"@en ;
    skos:broader eu-gdpr:DBIARiskStatus ;
    skos:definition "DBIA identifying high risk levels regarding rights and freedoms of natural persons"@en ;
    skos:inScheme eu-gdpr:data-breach-classes ;
    skos:prefLabel "DBIA Indicates High Risk"@en .

eu-gdpr:DBIAIndicatesLowRisk a rdfs:Class,
        skos:Concept,
        eu-gdpr:DBIARiskStatus ;
    dct:contributor _:N0a43dd9ea5e94fe695d8b7df8802cfdd ;
    dct:created "2024-05-19"^^xsd:date ;
    dct:source "GDPR Article 33"@en ;
    rdfs:isDefinedBy eu-gdpr: ;
    sw:term_status "accepted"@en ;
    skos:broader eu-gdpr:DBIARiskStatus ;
    skos:definition "DBIA identifying low risk levels regarding rights and freedoms of natural persons"@en ;
    skos:inScheme eu-gdpr:data-breach-classes ;
    skos:prefLabel "DBIA Indicates Low Risk"@en .

eu-gdpr:DBIAIndicatesNoRisk a rdfs:Class,
        skos:Concept,
        eu-gdpr:DBIARiskStatus ;
    dct:contributor _:N0a43dd9ea5e94fe695d8b7df8802cfdd ;
    dct:created "2024-05-19"^^xsd:date ;
    dct:source "GDPR Article 33"@en ;
    rdfs:isDefinedBy eu-gdpr: ;
    sw:term_status "accepted"@en ;
    skos:broader eu-gdpr:DBIARiskStatus ;
    skos:definition "DBIA identifying no risk is present regarding rights and freedoms of natural persons"@en ;
    skos:inScheme eu-gdpr:data-breach-classes ;
    skos:prefLabel "DBIA Indicates No Risk"@en .

eu-gdpr:DBIARiskStatus a rdfs:Class,
        skos:Concept ;
    dct:contributor _:N0a43dd9ea5e94fe695d8b7df8802cfdd ;
    dct:created "2024-05-19"^^xsd:date ;
    dct:source "GDPR Article 33"@en ;
    rdfs:isDefinedBy eu-gdpr: ;
    rdfs:subClassOf dpv:AuditStatus ;
    sw:term_status "accepted"@en ;
    skos:broader dpv:AuditStatus ;
    skos:definition "Status reflecting the status of risk associated with a DBIA regarding rights and freedoms of natural persons"@en ;
    skos:inScheme eu-gdpr:data-breach-classes ;
    skos:prefLabel "DBIA Risk Status"@en .

eu-gdpr:DPABreachInitialNotice a rdfs:Class,
        skos:Concept,
        eu-gdpr:DataBreachNotice ;
    dct:created "2024-05-19"^^xsd:date ;
    dct:source "GDPR Article 33"@en ;
    rdfs:isDefinedBy eu-gdpr: ;
    sw:term_status "accepted"@en ;
    skos:broader eu-gdpr:DPABreachNotice ;
    skos:definition "Notice sent by a Controller within 72 hours of becoming aware of a personal data breach to the competent DPA, with justifications provided where the notice is made after 72 hours"@en ;
    skos:inScheme eu-gdpr:data-breach-classes ;
    skos:prefLabel "DPA Breach Initial Notice"@en .

eu-gdpr:DPABreachNotice a rdfs:Class,
        skos:Concept,
        eu-gdpr:DataBreachNotice ;
    dct:created "2024-05-19"^^xsd:date ;
    dct:source "GDPR Article 33"@en ;
    rdfs:isDefinedBy eu-gdpr: ;
    sw:term_status "accepted"@en ;
    skos:broader eu-gdpr:DataBreachNotice ;
    skos:definition "Notice regarding a data breach to the DPA"@en ;
    skos:inScheme eu-gdpr:data-breach-classes ;
    skos:prefLabel "DPA Breach Notice"@en .

eu-gdpr:DPABreachNotificationNeeded a rdfs:Class,
        skos:Concept,
        eu-gdpr:DataBreachNoticeRequirement ;
    dct:contributor _:N0a43dd9ea5e94fe695d8b7df8802cfdd ;
    dct:created "2024-05-19"^^xsd:date ;
    dct:source "GDPR Article 33"@en ;
    rdfs:isDefinedBy eu-gdpr: ;
    sw:term_status "accepted"@en ;
    skos:broader eu-gdpr:DataBreachNoticeRequirement ;
    skos:definition "Data Breach notification to the DPA is required"@en ;
    skos:inScheme eu-gdpr:data-breach-classes ;
    skos:prefLabel "DPA Breach Notification Needed"@en .

eu-gdpr:DPABundledBreachNotice a rdfs:Class,
        skos:Concept,
        eu-gdpr:DataBreachNotice ;
    dct:created "2024-05-19"^^xsd:date ;
    dct:source "EDPB Guidelines 9/2022 on personal data breach notification under GDPR"@en ;
    rdfs:isDefinedBy eu-gdpr: ;
    sw:term_status "accepted"@en ;
    skos:broader eu-gdpr:DPABreachNotice ;
    skos:definition "Notice sent by a Controller to the DPA regarding multiple data breaches concerning the same type of personal data"@en ;
    skos:inScheme eu-gdpr:data-breach-classes ;
    skos:prefLabel "DPA Bundled Breach Notice"@en .

eu-gdpr:DPAPhasedBreachNotice a rdfs:Class,
        skos:Concept,
        eu-gdpr:DataBreachNotice ;
    dct:created "2024-05-19"^^xsd:date ;
    dct:source "EDPB Guidelines 9/2022 on personal data breach notification under GDPR"@en ;
    rdfs:isDefinedBy eu-gdpr: ;
    sw:term_status "accepted"@en ;
    skos:broader eu-gdpr:DPABreachNotice ;
    skos:definition "Notice sent to a DPA in phases i.e. by providing incremental information as it becomes available or is requested following previously submitted notifications"@en ;
    skos:inScheme eu-gdpr:data-breach-classes ;
    skos:prefLabel "DPA Phased Breach Notice"@en .

eu-gdpr:DPIAConformant a rdfs:Class,
        skos:Concept,
        eu-gdpr:DPIAConformity ;
    dct:contributor _:N05cd1f43dbaf4b4ba297dab5ee221394,
        _:N0a43dd9ea5e94fe695d8b7df8802cfdd ;
    dct:created "2022-10-22"^^xsd:date ;
    rdfs:isDefinedBy eu-gdpr: ;
    sw:term_status "accepted"@en ;
    skos:broader eu-gdpr:DPIAConformity ;
    skos:definition "Expressing the specified process is conformant with a DPIA"@en ;
    skos:inScheme eu-gdpr:dpia-classes ;
    skos:prefLabel "DPIA Conformant"@en .

eu-gdpr:DPIAConformity a rdfs:Class,
        skos:Concept ;
    dct:contributor _:N05cd1f43dbaf4b4ba297dab5ee221394,
        _:N0a43dd9ea5e94fe695d8b7df8802cfdd ;
    dct:created "2022-10-22"^^xsd:date ;
    rdfs:isDefinedBy eu-gdpr: ;
    rdfs:subClassOf dpv:ConformanceStatus ;
    sw:term_status "accepted"@en ;
    skos:broader dpv:ConformanceStatus ;
    skos:definition "Conformity of a process with a DPIA"@en ;
    skos:inScheme eu-gdpr:dpia-classes ;
    skos:prefLabel "DPIA Conformity"@en .

eu-gdpr:DPIAIndicatesHighRisk a rdfs:Class,
        skos:Concept,
        eu-gdpr:DPIARiskStatus ;
    dct:contributor _:N0a43dd9ea5e94fe695d8b7df8802cfdd ;
    dct:created "2022-06-22"^^xsd:date ;
    rdfs:isDefinedBy eu-gdpr: ;
    sw:term_status "accepted"@en ;
    skos:broader eu-gdpr:DPIARiskStatus ;
    skos:definition "DPIA identifying high risk levels"@en ;
    skos:inScheme eu-gdpr:dpia-classes ;
    skos:prefLabel "DPIA Indicates High Risk"@en .

eu-gdpr:DPIAIndicatesLowRisk a rdfs:Class,
        skos:Concept,
        eu-gdpr:DPIARiskStatus ;
    dct:contributor _:N0a43dd9ea5e94fe695d8b7df8802cfdd ;
    dct:created "2022-06-22"^^xsd:date ;
    rdfs:isDefinedBy eu-gdpr: ;
    sw:term_status "accepted"@en ;
    skos:broader eu-gdpr:DPIARiskStatus ;
    skos:definition "DPIA identifying low risk levels"@en ;
    skos:inScheme eu-gdpr:dpia-classes ;
    skos:prefLabel "DPIA Indicates Low Risk"@en .

eu-gdpr:DPIAIndicatesNoRisk a rdfs:Class,
        skos:Concept,
        eu-gdpr:DPIARiskStatus ;
    dct:contributor _:N0a43dd9ea5e94fe695d8b7df8802cfdd ;
    dct:created "2022-06-22"^^xsd:date ;
    rdfs:isDefinedBy eu-gdpr: ;
    sw:term_status "accepted"@en ;
    skos:broader eu-gdpr:DPIARiskStatus ;
    skos:definition "DPIA identifying no risk is present"@en ;
    skos:inScheme eu-gdpr:dpia-classes ;
    skos:prefLabel "DPIA Indicates No Risk"@en .

eu-gdpr:DPIANecessityAssessment a rdfs:Class,
        skos:Concept,
        dpv:OrganisationalMeasure ;
    dct:contributor _:N0a43dd9ea5e94fe695d8b7df8802cfdd ;
    dct:created "2022-06-22"^^xsd:date ;
    rdfs:isDefinedBy eu-gdpr: ;
    sw:term_status "accepted"@en ;
    skos:broader dpv:DPIA ;
    skos:definition "Process that determines whether a DPIA is necessary"@en ;
    skos:inScheme eu-gdpr:dpia-classes ;
    skos:prefLabel "DPIA Necessity Assessment"@en .

eu-gdpr:DPIANecessityStatus a rdfs:Class,
        skos:Concept ;
    dct:contributor _:N0a43dd9ea5e94fe695d8b7df8802cfdd ;
    dct:created "2022-06-22"^^xsd:date ;
    rdfs:isDefinedBy eu-gdpr: ;
    rdfs:subClassOf dpv:AuditStatus ;
    sw:term_status "accepted"@en ;
    skos:broader dpv:AuditStatus ;
    skos:definition "Status reflecting whether a DPIA is necessary"@en ;
    skos:inScheme eu-gdpr:dpia-classes ;
    skos:prefLabel "DPIA Necessity Status"@en .

eu-gdpr:DPIANonConformant a rdfs:Class,
        skos:Concept,
        eu-gdpr:DPIAConformity ;
    dct:contributor _:N05cd1f43dbaf4b4ba297dab5ee221394,
        _:N0a43dd9ea5e94fe695d8b7df8802cfdd ;
    dct:created "2022-10-22"^^xsd:date ;
    rdfs:isDefinedBy eu-gdpr: ;
    sw:term_status "accepted"@en ;
    skos:broader eu-gdpr:DPIAConformity ;
    skos:definition "Expressing the specified process is not conformant with a DPIA"@en ;
    skos:inScheme eu-gdpr:dpia-classes ;
    skos:prefLabel "DPIA Non-Conformant"@en .

eu-gdpr:DPIANotRequired a rdfs:Class,
        skos:Concept,
        eu-gdpr:DPIANecessityStatus ;
    dct:contributor _:N0a43dd9ea5e94fe695d8b7df8802cfdd ;
    dct:created "2022-06-22"^^xsd:date ;
    rdfs:isDefinedBy eu-gdpr: ;
    sw:term_status "accepted"@en ;
    skos:broader eu-gdpr:DPIANecessityStatus ;
    skos:definition "Condition where a DPIA is not required"@en ;
    skos:inScheme eu-gdpr:dpia-classes ;
    skos:prefLabel "DPIA Not Required"@en .

eu-gdpr:DPIAOutcome a rdfs:Class,
        skos:Concept,
        dpv:OrganisationalMeasure ;
    dct:contributor _:N0a43dd9ea5e94fe695d8b7df8802cfdd ;
    dct:created "2022-06-22"^^xsd:date ;
    rdfs:isDefinedBy eu-gdpr: ;
    sw:term_status "accepted"@en ;
    skos:broader dpv:DPIA ;
    skos:definition "Process representing determining outcome of a DPIA"@en ;
    skos:inScheme eu-gdpr:dpia-classes ;
    skos:prefLabel "DPIA Outcome"@en .

eu-gdpr:DPIAOutcomeDPAConsultation a rdfs:Class,
        skos:Concept,
        eu-gdpr:DPIAOutcomeStatus ;
    dct:contributor _:N0a43dd9ea5e94fe695d8b7df8802cfdd ;
    dct:created "2022-06-22"^^xsd:date ;
    rdfs:isDefinedBy eu-gdpr: ;
    sw:term_status "accepted"@en ;
    skos:broader eu-gdpr:DPIAOutcomeStatus ;
    skos:definition "DPIA outcome status indicating a DPA consultation is required"@en ;
    skos:inScheme eu-gdpr:dpia-classes ;
    skos:prefLabel "DPIA Outcome DPA Consultation"@en .

eu-gdpr:DPIAOutcomeHighResidualRisk a rdfs:Class,
        skos:Concept,
        eu-gdpr:DPIAOutcomeStatus ;
    dct:contributor _:N0a43dd9ea5e94fe695d8b7df8802cfdd ;
    dct:created "2022-06-22"^^xsd:date ;
    rdfs:isDefinedBy eu-gdpr: ;
    sw:term_status "accepted"@en ;
    skos:broader eu-gdpr:DPIAOutcomeStatus ;
    skos:definition "DPIA outcome status indicating high residual risk which are not acceptable for continuation"@en ;
    skos:inScheme eu-gdpr:dpia-classes ;
    skos:prefLabel "DPIA Outcome High Residual Risk"@en .

eu-gdpr:DPIAOutcomeRisksAcceptable a rdfs:Class,
        skos:Concept,
        eu-gdpr:DPIAOutcomeStatus ;
    dct:contributor _:N0a43dd9ea5e94fe695d8b7df8802cfdd ;
    dct:created "2024-05-19"^^xsd:date ;
    rdfs:isDefinedBy eu-gdpr: ;
    sw:term_status "accepted"@en ;
    skos:broader eu-gdpr:DPIAOutcomeStatus ;
    skos:definition "DPIA outcome status indicating residual risks remain and are acceptable for continuation"@en ;
    skos:inScheme eu-gdpr:dpia-classes ;
    skos:prefLabel "DPIA Outcome Risks Acceptable"@en .

eu-gdpr:DPIAOutcomeRisksMitigated a rdfs:Class,
        skos:Concept,
        eu-gdpr:DPIAOutcomeStatus ;
    dct:contributor _:N0a43dd9ea5e94fe695d8b7df8802cfdd ;
    dct:created "2022-06-22"^^xsd:date ;
    rdfs:isDefinedBy eu-gdpr: ;
    sw:term_status "accepted"@en ;
    skos:broader eu-gdpr:DPIAOutcomeStatus ;
    skos:definition "DPIA outcome status indicating (all) risks have been mitigated"@en ;
    skos:inScheme eu-gdpr:dpia-classes ;
    skos:prefLabel "DPIA Outcome Risks Mitigated"@en .

eu-gdpr:DPIAOutcomeStatus a rdfs:Class,
        skos:Concept ;
    dct:contributor _:N0a43dd9ea5e94fe695d8b7df8802cfdd ;
    dct:created "2022-06-22"^^xsd:date ;
    rdfs:isDefinedBy eu-gdpr: ;
    rdfs:subClassOf dpv:AuditStatus ;
    sw:term_status "accepted"@en ;
    skos:broader dpv:AuditStatus ;
    skos:definition "Status reflecting the outcomes of a DPIA"@en ;
    skos:inScheme eu-gdpr:dpia-classes ;
    skos:prefLabel "DPIA Outcome Status"@en .

eu-gdpr:DPIAProcedure a rdfs:Class,
        skos:Concept,
        dpv:OrganisationalMeasure ;
    dct:contributor _:N0a43dd9ea5e94fe695d8b7df8802cfdd ;
    dct:created "2022-06-22"^^xsd:date ;
    rdfs:isDefinedBy eu-gdpr: ;
    sw:term_status "accepted"@en ;
    skos:broader dpv:DPIA ;
    skos:definition "Process representing carrying out a DPIA"@en ;
    skos:inScheme eu-gdpr:dpia-classes ;
    skos:prefLabel "DPIA Procedure"@en .

eu-gdpr:DPIAProcessingRecommendation a rdfs:Class,
        skos:Concept ;
    dct:contributor _:N05cd1f43dbaf4b4ba297dab5ee221394,
        _:N0a43dd9ea5e94fe695d8b7df8802cfdd ;
    dct:created "2022-10-22"^^xsd:date ;
    rdfs:isDefinedBy eu-gdpr: ;
    rdfs:subClassOf dpv:AuditStatus ;
    sw:term_status "accepted"@en ;
    skos:broader dpv:AuditStatus ;
    skos:definition "Recommendation from the DPIA regarding processing"@en ;
    skos:inScheme eu-gdpr:dpia-classes ;
    skos:prefLabel "DPIA Processing Recommendation"@en .

eu-gdpr:DPIARecommendsProcessingContinue a rdfs:Class,
        skos:Concept,
        eu-gdpr:DPIAProcessingRecommendation ;
    dct:contributor _:N05cd1f43dbaf4b4ba297dab5ee221394,
        _:N0a43dd9ea5e94fe695d8b7df8802cfdd ;
    dct:created "2022-10-22"^^xsd:date ;
    rdfs:isDefinedBy eu-gdpr: ;
    sw:term_status "accepted"@en ;
    skos:broader eu-gdpr:DPIAProcessingRecommendation ;
    skos:definition "Recommendation from a DPIA that the processing may continue"@en ;
    skos:inScheme eu-gdpr:dpia-classes ;
    skos:prefLabel "DPIA Recommends Processing Continue"@en .

eu-gdpr:DPIARecommendsProcessingNotContinue a rdfs:Class,
        skos:Concept,
        eu-gdpr:DPIAProcessingRecommendation ;
    dct:contributor _:N05cd1f43dbaf4b4ba297dab5ee221394,
        _:N0a43dd9ea5e94fe695d8b7df8802cfdd ;
    dct:created "2022-10-22"^^xsd:date ;
    rdfs:isDefinedBy eu-gdpr: ;
    sw:term_status "accepted"@en ;
    skos:broader eu-gdpr:DPIAProcessingRecommendation ;
    skos:definition "Recommendation from a DPIA that the processing should not continue"@en ;
    skos:inScheme eu-gdpr:dpia-classes ;
    skos:prefLabel "DPIA Recommends Processing Not Continue"@en .

eu-gdpr:DPIARequired a rdfs:Class,
        skos:Concept,
        eu-gdpr:DPIANecessityStatus ;
    dct:contributor _:N0a43dd9ea5e94fe695d8b7df8802cfdd ;
    dct:created "2022-06-22"^^xsd:date ;
    rdfs:isDefinedBy eu-gdpr: ;
    sw:term_status "accepted"@en ;
    skos:broader eu-gdpr:DPIANecessityStatus ;
    skos:definition "Condition where a DPIA is required"@en ;
    skos:inScheme eu-gdpr:dpia-classes ;
    skos:prefLabel "DPIA Required"@en .

eu-gdpr:DPIARiskStatus a rdfs:Class,
        skos:Concept ;
    dct:contributor _:N0a43dd9ea5e94fe695d8b7df8802cfdd ;
    dct:created "2022-06-22"^^xsd:date ;
    rdfs:isDefinedBy eu-gdpr: ;
    rdfs:subClassOf dpv:AuditStatus ;
    sw:term_status "accepted"@en ;
    skos:broader dpv:AuditStatus ;
    skos:definition "Status reflecting the status of risk associated with a DPIA"@en ;
    skos:inScheme eu-gdpr:dpia-classes ;
    skos:prefLabel "DPIA Risk Status"@en .

eu-gdpr:DataBreach a rdfs:Class,
        skos:Concept ;
    dct:created "2024-05-19"^^xsd:date ;
    dct:source "GDPR Article 4(12)"@en ;
    rdfs:isDefinedBy eu-gdpr: ;
    rdfs:subClassOf risk:Incident ;
    sw:term_status "accepted"@en ;
    skos:broader risk:Incident ;
    skos:definition "Data Breach' or ‘Personal Data Breach’ means a breach of security leading to the accidental or unlawful destruction, loss, alteration, unauthorised disclosure of, or access to, personal data transmitted, stored or otherwise processed"@en ;
    skos:inScheme eu-gdpr:data-breach-classes ;
    skos:prefLabel "Data Breach"@en ;
    skos:scopeNote "GDPR's notion of data breach includes any incident that affects the confidentiality, integrity, and availability of personal data and its processing without distinguishing between internal or external actors involved in the incident"@en .

eu-gdpr:DataBreachConcludingReport a rdfs:Class,
        skos:Concept ;
    dct:created "2024-05-19"^^xsd:date ;
    dct:source "GDPR Article 33"@en ;
    rdfs:isDefinedBy eu-gdpr: ;
    rdfs:subClassOf eu-gdpr:DataBreachReport,
        risk:IncidentHandlingReport ;
    sw:term_status "accepted"@en ;
    skos:broader eu-gdpr:DataBreachReport,
        risk:IncidentHandlingReport ;
    skos:definition "Documented information about a concluded data breach incident"@en ;
    skos:inScheme eu-gdpr:data-breach-classes ;
    skos:prefLabel "Data Breach Concluding Report"@en .

eu-gdpr:DataBreachDetectionReport a rdfs:Class,
        skos:Concept ;
    dct:created "2024-05-19"^^xsd:date ;
    dct:source "GDPR Article 33"@en ;
    rdfs:isDefinedBy eu-gdpr: ;
    rdfs:subClassOf eu-gdpr:DataBreachReport,
        risk:IncidentDetectionReport ;
    sw:term_status "accepted"@en ;
    skos:broader eu-gdpr:DataBreachReport,
        risk:IncidentDetectionReport ;
    skos:definition "Documented information about a data breach being detected"@en ;
    skos:inScheme eu-gdpr:data-breach-classes ;
    skos:prefLabel "Data Breach Detection Report"@en .

eu-gdpr:DataBreachJustification a rdfs:Class,
        skos:Concept,
        dpv:Justification ;
    dct:contributor _:N05cd1f43dbaf4b4ba297dab5ee221394,
        _:N0a43dd9ea5e94fe695d8b7df8802cfdd,
        _:N458008bc6195484e9cc557f70eabda31 ;
    dct:created "2024-12-17"^^xsd:date ;
    rdfs:isDefinedBy eu-gdpr: ;
    sw:term_status "accepted"@en ;
    skos:broader dpv:Justification ;
    skos:definition "A Justification used in the context of data breach related processes and communications"@en ;
    skos:inScheme eu-gdpr:data-breach-classes ;
    skos:prefLabel "Data Breach Justification"@en .

eu-gdpr:DataBreachNotice a rdfs:Class,
        skos:Concept ;
    dct:created "2024-05-19"^^xsd:date ;
    dct:source "GDPR Article 33"@en ;
    rdfs:isDefinedBy eu-gdpr: ;
    rdfs:subClassOf dpv:DataBreachNotice ;
    sw:term_status "accepted"@en ;
    skos:broader dpv:DataBreachNotice ;
    skos:definition "Notice associated with data breach providing information in compliance with GDPR"@en ;
    skos:inScheme eu-gdpr:data-breach-classes ;
    skos:prefLabel "Data Breach Notice"@en .

eu-gdpr:DataBreachNoticeRequirement a rdfs:Class,
        skos:Concept ;
    dct:contributor _:N0a43dd9ea5e94fe695d8b7df8802cfdd ;
    dct:created "2024-05-19"^^xsd:date ;
    dct:source "GDPR Article 33"@en ;
    rdfs:isDefinedBy eu-gdpr: ;
    rdfs:subClassOf dpv:AuditStatus ;
    sw:term_status "accepted"@en ;
    skos:broader dpv:AuditStatus ;
    skos:definition "Whether a Data Breach notification is required"@en ;
    skos:inScheme eu-gdpr:data-breach-classes ;
    skos:prefLabel "Data Breach Notice Requirement"@en .

eu-gdpr:DataBreachOngoingReport a rdfs:Class,
        skos:Concept ;
    dct:created "2024-05-19"^^xsd:date ;
    dct:source "GDPR Article 33"@en ;
    rdfs:isDefinedBy eu-gdpr: ;
    rdfs:subClassOf eu-gdpr:DataBreachReport,
        risk:IncidentAssessmentReport ;
    sw:term_status "accepted"@en ;
    skos:broader eu-gdpr:DataBreachReport,
        risk:IncidentAssessmentReport ;
    skos:definition "Documented information about an ongoing data breach"@en ;
    skos:inScheme eu-gdpr:data-breach-classes ;
    skos:prefLabel "Data Breach Ongoing Report"@en .

eu-gdpr:DataBreachPreliminaryReport a rdfs:Class,
        skos:Concept ;
    dct:created "2024-05-19"^^xsd:date ;
    dct:source "GDPR Article 33"@en ;
    rdfs:isDefinedBy eu-gdpr: ;
    rdfs:subClassOf eu-gdpr:DataBreachReport,
        risk:IncidentAssessmentReport ;
    sw:term_status "accepted"@en ;
    skos:broader eu-gdpr:DataBreachReport,
        risk:IncidentAssessmentReport ;
    skos:definition "Documented information about preliminary assessment regarding a data breach"@en ;
    skos:inScheme eu-gdpr:data-breach-classes ;
    skos:prefLabel "Data Breach Preliminary Report"@en .

eu-gdpr:DataBreachRegister a rdfs:Class,
        skos:Concept ;
    dct:created "2024-05-19"^^xsd:date ;
    dct:source "GDPR Article 33(5)"@en ;
    rdfs:isDefinedBy eu-gdpr: ;
    rdfs:subClassOf dpv:RecordsOfActivities ;
    sw:term_status "accepted"@en ;
    skos:broader dpv:RecordsOfActivities ;
    skos:definition "Register of data breaches containing facts relating to the personal data breach, its effects and the remedial action taken"@en ;
    skos:inScheme eu-gdpr:data-breach-classes ;
    skos:prefLabel "Data Breach Register"@en .

eu-gdpr:DataBreachReport a rdfs:Class,
        skos:Concept ;
    dct:created "2024-05-19"^^xsd:date ;
    dct:source "GDPR Article 33"@en ;
    rdfs:isDefinedBy eu-gdpr: ;
    rdfs:subClassOf risk:IncidentReport ;
    sw:term_status "accepted"@en ;
    skos:broader risk:IncidentReport ;
    skos:definition "Documented information about a data breach incident, its handling, assessments, and notifications"@en ;
    skos:inScheme eu-gdpr:data-breach-classes ;
    skos:prefLabel "Data Breach Report"@en .

eu-gdpr:DataMinimisationPrinciple a rdfs:Class,
        skos:Concept,
        dpv:OrganisationalMeasure ;
    dct:contributor _:N05cd1f43dbaf4b4ba297dab5ee221394 ;
    dct:created "2024-05-12"^^xsd:date ;
    dct:source "GDPR Art.5-1c"@en ;
    rdfs:isDefinedBy eu-gdpr: ;
    sw:term_status "accepted"@en ;
    skos:broader dpv:Principle ;
    skos:definition "Principle stating personal data must be processed adequate, relevant and limited to what is necessary in relation to the purposes for which they are processed"@en ;
    skos:inScheme eu-gdpr:principles-classes ;
    skos:prefLabel "Data Minimisation Principle"@en .

eu-gdpr:DataProtectionAuthority a rdfs:Class,
        skos:Concept ;
    dct:contributor _:N05cd1f43dbaf4b4ba297dab5ee221394,
        _:N0a43dd9ea5e94fe695d8b7df8802cfdd ;
    dct:created "2024-06-22"^^xsd:date ;
    dct:source " Guidelines 3/2018 on the territorial scope of the GDPR (Article 3) Version 2.1"@en,
        "GDPR Art.56"@en ;
    rdfs:isDefinedBy eu-gdpr: ;
    rdfs:subClassOf dpv:DataProtectionAuthority ;
    sw:term_status "accepted"@en ;
    skos:broader dpv:DataProtectionAuthority ;
    skos:definition "‘Supervisory Authority’ or 'Data Protection Authority' means an independent public authority which is established by a Member State pursuant to Article 51"@en ;
    skos:inScheme eu-gdpr:entities-classes ;
    skos:prefLabel "Data Protection Authority"@en .

eu-gdpr:DataSubject a rdfs:Class,
        skos:Concept ;
    dct:contributor _:N0a43dd9ea5e94fe695d8b7df8802cfdd ;
    dct:created "2024-12-17"^^xsd:date ;
    dct:source "GDPR Art.4-1"@en ;
    rdfs:isDefinedBy eu-gdpr: ;
    rdfs:subClassOf dpv:DataSubject ;
    sw:term_status "accepted"@en ;
    skos:broader dpv:DataSubject ;
    skos:definition "Data Subject' means a natural person who can be identified, directly or indirectly, in particular by reference to an identifier such as a name, an identification number, location data, an online identifier or to one or more factors specific to the physical, physiological, genetic, mental, economic, cultural or social identity of that natural person"@en ;
    skos:inScheme eu-gdpr:entities-classes ;
    skos:prefLabel "Data Subject"@en .

eu-gdpr:DataSubjectBreachNotice a rdfs:Class,
        skos:Concept,
        eu-gdpr:DataBreachNotice ;
    dct:created "2024-05-19"^^xsd:date ;
    dct:source "GDPR Article 34"@en ;
    rdfs:isDefinedBy eu-gdpr: ;
    sw:term_status "accepted"@en ;
    skos:broader eu-gdpr:DataBreachNotice ;
    skos:definition "Notice regarding a data breach to the Data Subject"@en ;
    skos:inScheme eu-gdpr:data-breach-classes ;
    skos:prefLabel "Data Subject Breach Notice"@en .

eu-gdpr:DataSubjectBreachNotificationNeeded a rdfs:Class,
        skos:Concept,
        eu-gdpr:DataBreachNoticeRequirement ;
    dct:created "2024-05-19"^^xsd:date ;
    dct:source "GDPR Article 34"@en ;
    rdfs:isDefinedBy eu-gdpr: ;
    sw:term_status "accepted"@en ;
    skos:broader eu-gdpr:DataBreachNoticeRequirement ;
    skos:definition "Data Breach notification to the Data Subject is required"@en ;
    skos:inScheme eu-gdpr:data-breach-classes ;
    skos:prefLabel "Data Subject Breach Notification Needed"@en .

eu-gdpr:DataTransferTool a rdfs:Class,
        skos:Concept,
        dpv:OrganisationalMeasure ;
    dct:contributor _:N0a43dd9ea5e94fe695d8b7df8802cfdd,
        _:N1aa8f48a4f3a40e6a438f71be918d3a1 ;
    dct:created "2021-09-22"^^xsd:date ;
    dct:modified "2023-10-30"^^xsd:date ;
    dct:source [ a schema:WebPage ;
            schema:name "GDPR Art.46 and EDPB Recommendations 01/2020 on Supplementary Measures and Transfer Tools" ;
            schema:url "https://edpb.europa.eu/sites/default/files/consultation/edpb_recommendations_202001_supplementarymeasurestransferstools_en.pdf" ] ;
    rdfs:isDefinedBy eu-gdpr: ;
    sw:term_status "accepted"@en ;
    skos:broader dpv:OrganisationalMeasure ;
    skos:definition "A legal instrument or tool intended to assist or justify data transfers"@en ;
    skos:inScheme eu-gdpr:data-transfers-classes ;
    skos:prefLabel "Data Transfer Tool"@en .

eu-gdpr:DirectDataCollectionNotice a rdfs:Class,
        skos:Concept,
        dpv:OrganisationalMeasure ;
    dct:contributor _:N05cd1f43dbaf4b4ba297dab5ee221394,
        _:N0a43dd9ea5e94fe695d8b7df8802cfdd,
        _:N458008bc6195484e9cc557f70eabda31 ;
    dct:created "2022-11-09"^^xsd:date ;
    rdfs:isDefinedBy eu-gdpr: ;
    sw:term_status "accepted"@en ;
    skos:broader dpv:RightFulfilmentNotice ;
    skos:definition "A Notice provided in fulfilment of GDPR's Art.13 regarding information to be provided where personal data are collected from the data subject"@en ;
    skos:inScheme eu-gdpr:rights-classes ;
    skos:prefLabel "Direct Data Collection Notice"@en .

eu-gdpr:Establishment a rdfs:Class,
        skos:Concept ;
    dct:contributor _:N05cd1f43dbaf4b4ba297dab5ee221394,
        _:N0a43dd9ea5e94fe695d8b7df8802cfdd ;
    dct:created "2024-02-14"^^xsd:date ;
    dct:source " GDPR Art.56"@en,
        " Guidelines 3/2018 on the territorial scope of the GDPR (Article 3) Version 2.1"@en,
        "GDPR Recital 22"@en ;
    rdfs:isDefinedBy eu-gdpr: ;
    rdfs:subClassOf dpv:Organisation ;
    sw:term_status "accepted"@en ;
    skos:broader dpv:Organisation ;
    skos:definition "Establishment is a Legal Entity which implies the effective and real exercise of activities through stable arrangements (with a presumed parent or primary establishment)"@en ;
    skos:inScheme eu-gdpr:entities-classes ;
    skos:prefLabel "Establishment"@en .

eu-gdpr:FairnessPrinciple a rdfs:Class,
        skos:Concept,
        dpv:OrganisationalMeasure ;
    dct:contributor _:N05cd1f43dbaf4b4ba297dab5ee221394 ;
    dct:created "2024-05-12"^^xsd:date ;
    dct:source "GDPR Art.5-1a"@en ;
    rdfs:isDefinedBy eu-gdpr: ;
    sw:term_status "accepted"@en ;
    skos:broader dpv:Principle ;
    skos:definition "Principle stating personal data must be processed processed fairly in relation to the data subject"@en ;
    skos:inScheme eu-gdpr:principles-classes ;
    skos:prefLabel "Fairness Principle"@en .

eu-gdpr:GDPRComplianceUnknown a rdfs:Class,
        skos:Concept,
        dpv:Lawfulness ;
    dct:contributor _:N0a43dd9ea5e94fe695d8b7df8802cfdd ;
    dct:created "2022-10-22"^^xsd:date ;
    rdfs:isDefinedBy eu-gdpr: ;
    sw:term_status "accepted"@en ;
    skos:broader eu-gdpr:GDPRLawfulness ;
    skos:definition "State where lawfulness or compliance with GDPR is unknown"@en ;
    skos:inScheme eu-gdpr:compliance-classes ;
    skos:prefLabel "GDPR Compliance Unknown"@en .

eu-gdpr:GDPRCompliant a rdfs:Class,
        skos:Concept,
        dpv:Lawfulness ;
    dct:contributor _:N0a43dd9ea5e94fe695d8b7df8802cfdd ;
    dct:created "2022-10-22"^^xsd:date ;
    rdfs:isDefinedBy eu-gdpr: ;
    sw:term_status "accepted"@en ;
    skos:broader eu-gdpr:GDPRLawfulness ;
    skos:definition "State of being lawful or legally compliant for GDPR"@en ;
    skos:inScheme eu-gdpr:compliance-classes ;
    skos:prefLabel "GDPR Compliant"@en .

eu-gdpr:GDPRLawfulness a rdfs:Class,
        skos:Concept,
        dpv:Lawfulness ;
    dct:contributor _:N0a43dd9ea5e94fe695d8b7df8802cfdd ;
    dct:created "2022-10-22"^^xsd:date ;
    vann:example dex:E0055 ;
    rdfs:isDefinedBy eu-gdpr: ;
    sw:term_status "accepted"@en ;
    skos:broader dpv:Lawfulness ;
    skos:definition "Status or state associated with being lawful or legally compliant regarding GDPR"@en ;
    skos:inScheme eu-gdpr:compliance-classes ;
    skos:prefLabel "GDPR Lawfulness"@en .

eu-gdpr:GDPRNonCompliant a rdfs:Class,
        skos:Concept,
        dpv:Lawfulness ;
    dct:contributor _:N0a43dd9ea5e94fe695d8b7df8802cfdd ;
    dct:created "2022-10-22"^^xsd:date ;
    rdfs:isDefinedBy eu-gdpr: ;
    sw:term_status "accepted"@en ;
    skos:broader eu-gdpr:GDPRLawfulness ;
    skos:definition "State of being unlawful or legally non-compliant for GDPR"@en ;
    skos:inScheme eu-gdpr:compliance-classes ;
    skos:prefLabel "GDPR Non-compliant"@en .

eu-gdpr:GDPRRightsImpact a rdfs:Class,
        skos:Concept,
        risk:PotentialConsequence,
        risk:PotentialImpact,
        risk:PotentialRisk,
        risk:RiskConcept ;
    dct:created "2024-12-01"^^xsd:date ;
    rdfs:isDefinedBy eu-gdpr: ;
    sw:term_status "accepted"@en ;
    skos:broader risk:RightsImpact ;
    skos:definition "Something that acts as or is considered as an impact on one or more rights defined by GDPR"@en ;
    skos:inScheme eu-gdpr:rights-impacts-classes ;
    skos:prefLabel "GDPR Rights Impact"@en .

eu-gdpr:GeneticData a rdfs:Class,
        skos:Concept,
        pd:Genetic ;
    dct:contributor _:N0a43dd9ea5e94fe695d8b7df8802cfdd ;
    dct:created "2024-12-17"^^xsd:date ;
    rdf:value "dpv:PersonalData" ;
    rdfs:isDefinedBy eu-gdpr: ;
    sw:term_status "accepted"@en ;
    skos:broader pd:Genetic ;
    skos:definition "‘Genetic Data’ means personal data relating to the inherited or acquired genetic characteristics of a natural person which give unique information about the physiology or the health of that natural person and which result, in particular, from an analysis of a biological sample from the natural person in question"@en ;
    skos:inScheme eu-gdpr:misc-concepts-classes ;
    skos:prefLabel "Genetic Data"@en .

eu-gdpr:HealthData a rdfs:Class,
        skos:Concept,
        pd:MedicalHealth ;
    dct:contributor _:N0a43dd9ea5e94fe695d8b7df8802cfdd ;
    dct:created "2024-12-17"^^xsd:date ;
    rdf:value "dpv:PersonalData" ;
    rdfs:isDefinedBy eu-gdpr: ;
    sw:term_status "accepted"@en ;
    skos:broader pd:MedicalHealth ;
    skos:definition "Health Data' or 'data concerning health’ means personal data related to the physical or mental health of a natural person, including the provision of health care services, which reveal information about his or her health status"@en ;
    skos:inScheme eu-gdpr:misc-concepts-classes ;
    skos:prefLabel "Health Data"@en .

eu-gdpr:IndirectDataCollectionNotice a rdfs:Class,
        skos:Concept,
        dpv:OrganisationalMeasure ;
    dct:contributor _:N05cd1f43dbaf4b4ba297dab5ee221394,
        _:N0a43dd9ea5e94fe695d8b7df8802cfdd,
        _:N458008bc6195484e9cc557f70eabda31 ;
    dct:created "2022-11-09"^^xsd:date ;
    rdfs:isDefinedBy eu-gdpr: ;
    sw:term_status "accepted"@en ;
    skos:broader dpv:RightFulfilmentNotice ;
    skos:definition "A Notice provided in fulfilment of GDPR's Art.14 regarding information to be provided where personal data are not collected from the data subject"@en ;
    skos:inScheme eu-gdpr:rights-classes ;
    skos:prefLabel "Indirect Data Collection Notice"@en .

eu-gdpr:InformationSocietyService a rdfs:Class,
        skos:Concept,
        dpv:Service ;
    dct:contributor _:N0a43dd9ea5e94fe695d8b7df8802cfdd ;
    dct:created "2024-12-17"^^xsd:date ;
    rdf:value "sc" ;
    rdfs:isDefinedBy eu-gdpr: ;
    sw:term_status "accepted"@en ;
    skos:broader dpv:Service ;
    skos:definition "Information Society Service’ means a service as defined in point (b) of Article 1(1) of Directive (EU) 2015/1535 of the European Parliament and of the Council"@en ;
    skos:inScheme eu-gdpr:misc-concepts-classes ;
    skos:prefLabel "Information Society Service"@en .

eu-gdpr:IntegrityBreach a rdfs:Class,
        skos:Concept ;
    dct:created "2024-05-19"^^xsd:date ;
    dct:source "EDPB Guidelines 9/2022 on personal data breach notification under GDPR"@en ;
    rdfs:isDefinedBy eu-gdpr: ;
    rdfs:subClassOf eu-gdpr:DataBreach ;
    sw:term_status "accepted"@en ;
    skos:broader eu-gdpr:DataBreach ;
    skos:definition "A data breach where there is an unauthorised or accidental alteration of personal data"@en ;
    skos:inScheme eu-gdpr:data-breach-classes ;
    skos:prefLabel "Integrity Breach"@en .

eu-gdpr:IntegrityConfidentialityPrinciple a rdfs:Class,
        skos:Concept,
        dpv:OrganisationalMeasure ;
    dct:contributor _:N05cd1f43dbaf4b4ba297dab5ee221394 ;
    dct:created "2024-05-12"^^xsd:date ;
    dct:source "GDPR Art.5-1f"@en ;
    rdfs:isDefinedBy eu-gdpr: ;
    sw:term_status "accepted"@en ;
    skos:broader dpv:Principle ;
    skos:definition "Principle stating personal data must be processed in a manner that ensures appropriate security of the personal data, including protection against unauthorised or unlawful processing and against accidental loss, destruction or damage, using appropriate technical or organisational measures"@en ;
    skos:inScheme eu-gdpr:principles-classes ;
    skos:prefLabel "Integrity Confidentiality Principle"@en .

eu-gdpr:InternationalOrganisation a rdfs:Class,
        skos:Concept ;
    dct:contributor _:N0a43dd9ea5e94fe695d8b7df8802cfdd ;
    dct:created "2024-12-17"^^xsd:date ;
    dct:source "GDPR Art.4-26"@en ;
    rdfs:isDefinedBy eu-gdpr: ;
    rdfs:subClassOf dpv:InternationalOrganisation ;
    sw:term_status "accepted"@en ;
    skos:broader dpv:InternationalOrganisation ;
    skos:definition "‘International Organisation’ means an organisation and its subordinate bodies governed by public international law, or any other body which is set up by, or on the basis of, an agreement between two or more countries"@en ;
    skos:inScheme eu-gdpr:entities-classes ;
    skos:prefLabel "International Organisation"@en .

eu-gdpr:JustificationA12Complexity a rdfs:Class,
        skos:Concept,
        dpv:Justification ;
    dct:contributor _:N05cd1f43dbaf4b4ba297dab5ee221394,
        _:N0a43dd9ea5e94fe695d8b7df8802cfdd,
        _:N458008bc6195484e9cc557f70eabda31 ;
    dct:created "2024-12-17"^^xsd:date ;
    dct:source "GDPR Art.12-3"@en ;
    rdfs:isDefinedBy eu-gdpr: ;
    sw:term_status "accepted"@en ;
    skos:broader justifications:ComplexityOfProcess,
        eu-gdpr:JustificationA12Delay ;
    skos:definition "Justification that the request under A15-A22 is delayed due to complexity in fulfilling it"@en ;
    skos:inScheme eu-gdpr:rights-justifications-classes ;
    skos:prefLabel "Justification A12 - Complexity"@en .

eu-gdpr:JustificationA12Delay a rdfs:Class,
        skos:Concept,
        dpv:Justification ;
    dct:contributor _:N05cd1f43dbaf4b4ba297dab5ee221394,
        _:N0a43dd9ea5e94fe695d8b7df8802cfdd,
        _:N458008bc6195484e9cc557f70eabda31 ;
    dct:created "2024-12-17"^^xsd:date ;
    dct:source "GDPR Art.12-3"@en ;
    rdfs:isDefinedBy eu-gdpr: ;
    sw:term_status "accepted"@en ;
    skos:broader justifications:DelayJustification ;
    skos:definition "Justification that the request under A15-A22 is delayed"@en ;
    skos:inScheme eu-gdpr:rights-justifications-classes ;
    skos:prefLabel "Justification A12 - Delay"@en ;
    skos:scopeNote "The justification is for when the initial process, which is to be completed within one month of receipt of the request, is delayed with Art.12-3 stating a duration of two further months where necessary taking into account the complexity and number of the requests. In such cases, the controller is needed to inform the data subject of the extension within one month of receipt of the request together with the reasons for the delay - which is done through this extension. Information about expected duration of response can be provided through use of dpv:hasDuration. The specific nature of delay can be expressed through use of eu-gdpr:A12ComplexityOfRequest or eu-gdpr:A12HighVolumeOfRequest"@en .

eu-gdpr:JustificationA12HighVolume a rdfs:Class,
        skos:Concept,
        dpv:Justification ;
    dct:contributor _:N05cd1f43dbaf4b4ba297dab5ee221394,
        _:N0a43dd9ea5e94fe695d8b7df8802cfdd,
        _:N458008bc6195484e9cc557f70eabda31 ;
    dct:created "2024-12-17"^^xsd:date ;
    dct:source "GDPR Art.12-3"@en ;
    rdfs:isDefinedBy eu-gdpr: ;
    sw:term_status "accepted"@en ;
    skos:broader justifications:HighVolumeOfProcesses,
        eu-gdpr:JustificationA12Delay ;
    skos:definition "Justification that the request under A15-A22 is delayed due to high volume of similar requestes required to be fulfilled"@en ;
    skos:inScheme eu-gdpr:rights-justifications-classes ;
    skos:prefLabel "Justification A12 - High Volume"@en .

eu-gdpr:JustificationA12IdentityFailure a rdfs:Class,
        skos:Concept,
        dpv:Justification ;
    dct:contributor _:N05cd1f43dbaf4b4ba297dab5ee221394,
        _:N0a43dd9ea5e94fe695d8b7df8802cfdd,
        _:N458008bc6195484e9cc557f70eabda31 ;
    dct:created "2024-12-17"^^xsd:date ;
    dct:source "GDPR Art.12-6"@en ;
    rdfs:isDefinedBy eu-gdpr: ;
    sw:term_status "accepted"@en ;
    skos:broader justifications:IdentityVerificationFailure ;
    skos:definition "Justification that a request under A14-21 could not be fulfiled due to lack of identity verification"@en ;
    skos:inScheme eu-gdpr:rights-justifications-classes ;
    skos:prefLabel "Justification A12 - Identity Failure"@en ;
    skos:scopeNote "For justifications where identity cannot be verified and requires additional information, eu-gdpr:A12IdentityVerificationRequired should be used"@en .

eu-gdpr:JustificationA12IdentityRequired a rdfs:Class,
        skos:Concept,
        dpv:Justification ;
    dct:contributor _:N05cd1f43dbaf4b4ba297dab5ee221394,
        _:N0a43dd9ea5e94fe695d8b7df8802cfdd,
        _:N458008bc6195484e9cc557f70eabda31 ;
    dct:created "2024-12-17"^^xsd:date ;
    dct:source "GDPR Art.12-6"@en ;
    rdfs:isDefinedBy eu-gdpr: ;
    sw:term_status "accepted"@en ;
    skos:broader justifications:IdentityVerificationRequired ;
    skos:definition "Justification that a request under A14-21 could not be fulfiled due to lack of identity verification, and therefore requires additional information to complete the identity verification request"@en ;
    skos:inScheme eu-gdpr:rights-justifications-classes ;
    skos:prefLabel "Justification A12 - Identity Required"@en ;
    skos:scopeNote "If the purpose of this justification is to ask for identity verification, then it requires information on what information is considered as an accepable form of identity, which can ideally be expressed through dpv:Process and relevant dpv:PersonalData categories, or through a comment or description for the justification"@en .

eu-gdpr:JustificationA12InformationRequired a rdfs:Class,
        skos:Concept,
        dpv:Justification ;
    dct:contributor _:N05cd1f43dbaf4b4ba297dab5ee221394,
        _:N0a43dd9ea5e94fe695d8b7df8802cfdd,
        _:N458008bc6195484e9cc557f70eabda31 ;
    dct:created "2024-12-17"^^xsd:date ;
    dct:source "GDPR Art.12-6"@en ;
    rdfs:isDefinedBy eu-gdpr: ;
    sw:term_status "accepted"@en ;
    skos:broader justifications:InformationRequired ;
    skos:definition "Justification that the request under A14-21 could not be fulfilled due to additional information being required"@en ;
    skos:inScheme eu-gdpr:rights-justifications-classes ;
    skos:prefLabel "Justification A12 - Information Required"@en ;
    skos:scopeNote "If the purpose of this justification is to ask for identity verification, then eu-gdpr:A12IdentityVerificationRequired should be used. The information required can be expressed using dpv:Process, which allows also expressing the purpose for why it is required and relevant dpv:PersonalData categories, or through a comment or description for the justification"@en .

eu-gdpr:JustificationA12LackOfIntent a rdfs:Class,
        skos:Concept,
        dpv:Justification ;
    dct:contributor _:N05cd1f43dbaf4b4ba297dab5ee221394,
        _:N0a43dd9ea5e94fe695d8b7df8802cfdd,
        _:N458008bc6195484e9cc557f70eabda31 ;
    dct:created "2024-12-17"^^xsd:date ;
    dct:source "GDPR Art.12-5"@en ;
    rdfs:isDefinedBy eu-gdpr: ;
    sw:term_status "accepted"@en ;
    skos:broader justifications:LackOfIntent,
        eu-gdpr:JustificationA12ManifestlyUnfounded ;
    skos:definition "Justification that a request under A13-A22 and A34 is manifestly unfounded - in particular due to a lack of intent - and therefore is being charged a fee or is being refused"@en ;
    skos:inScheme eu-gdpr:rights-justifications-classes ;
    skos:prefLabel "Justification A12 - Lack Of Intent"@en ;
    skos:scopeNote "This justification requires information on why or how the lack of intent was assessed, which can be provided as a description of comment"@en .

eu-gdpr:JustificationA12MaliciousIntent a rdfs:Class,
        skos:Concept,
        dpv:Justification ;
    dct:contributor _:N05cd1f43dbaf4b4ba297dab5ee221394,
        _:N0a43dd9ea5e94fe695d8b7df8802cfdd,
        _:N458008bc6195484e9cc557f70eabda31 ;
    dct:created "2024-12-17"^^xsd:date ;
    dct:source "GDPR Art.12-5"@en ;
    rdfs:isDefinedBy eu-gdpr: ;
    sw:term_status "accepted"@en ;
    skos:broader justifications:ProcessMalicious,
        eu-gdpr:JustificationA12ManifestlyUnfounded ;
    skos:definition "Justification that a request under A13-A22 and A34 is manifestly unfounded - in particular due to malicious intent - and therefore is being charged a fee or is being refused"@en ;
    skos:inScheme eu-gdpr:rights-justifications-classes ;
    skos:prefLabel "Justification A12 - Malicious Intent"@en ;
    skos:scopeNote "This justification requires information on why or how the malicious intent was assessed, which can be provided as a description of comment"@en .

eu-gdpr:JustificationA12ManifestlyExcessive a rdfs:Class,
        skos:Concept,
        dpv:Justification ;
    dct:contributor _:N05cd1f43dbaf4b4ba297dab5ee221394,
        _:N0a43dd9ea5e94fe695d8b7df8802cfdd,
        _:N458008bc6195484e9cc557f70eabda31 ;
    dct:created "2024-12-17"^^xsd:date ;
    dct:source "GDPR Art.12-5"@en ;
    rdfs:isDefinedBy eu-gdpr: ;
    sw:term_status "accepted"@en ;
    skos:broader justifications:ProcessExcessive ;
    skos:definition "Justification that a request under A13-A22 and A34 is manifestly excessive and therefore is being charged a fee or is being refused"@en ;
    skos:inScheme eu-gdpr:rights-justifications-classes ;
    skos:prefLabel "Justification A12 - Manifestly Excessive"@en ;
    skos:scopeNote "This justification requires information on why or how the assessment of manifestly excessive was made, which can be provided as a description of comment"@en .

eu-gdpr:JustificationA12ManifestlyUnfounded a rdfs:Class,
        skos:Concept,
        dpv:Justification ;
    dct:contributor _:N05cd1f43dbaf4b4ba297dab5ee221394,
        _:N0a43dd9ea5e94fe695d8b7df8802cfdd,
        _:N458008bc6195484e9cc557f70eabda31 ;
    dct:created "2024-12-17"^^xsd:date ;
    dct:source "GDPR Art.12-5"@en ;
    rdfs:isDefinedBy eu-gdpr: ;
    sw:term_status "accepted"@en ;
    skos:broader justifications:ProcessUnfounded ;
    skos:definition "Justification that a process under A13-A22 and A34 is manifestly unfounded and therefore is being charged a fee or is being refused"@en ;
    skos:inScheme eu-gdpr:rights-justifications-classes ;
    skos:prefLabel "Justification A12 - Manifestly Unfounded"@en ;
    skos:scopeNote "This justification requires information on why the process was considered manifestly unfounded which can be expressed through the additional concepts provided such as eu-gdpr:A12LackOfIntent or eu-gdpr:A12MaliciousIntent, or which can be provided as a description of comment"@en .

eu-gdpr:JustificationA13EntityAlreadyInformed a rdfs:Class,
        skos:Concept,
        dpv:Justification ;
    dct:contributor _:N05cd1f43dbaf4b4ba297dab5ee221394,
        _:N0a43dd9ea5e94fe695d8b7df8802cfdd,
        _:N458008bc6195484e9cc557f70eabda31 ;
    dct:created "2024-12-17"^^xsd:date ;
    dct:source "GDPR Art.13-4"@en ;
    rdfs:isDefinedBy eu-gdpr: ;
    sw:term_status "accepted"@en ;
    skos:broader justifications:EntityAlreadyInformed ;
    skos:definition "Justification that A13 obligations for providing information do not apply as the data subject already has the information"@en ;
    skos:inScheme eu-gdpr:rights-justifications-classes ;
    skos:prefLabel "Justification A13 - Entity Already Informed"@en ;
    skos:scopeNote "This justification requires information on how the data subject was provided the information to satify the assertion, which can be provided as a description of comment"@en .

eu-gdpr:JustificationA14ConfidentialityCompromised a rdfs:Class,
        skos:Concept,
        dpv:Justification ;
    dct:contributor _:N05cd1f43dbaf4b4ba297dab5ee221394,
        _:N0a43dd9ea5e94fe695d8b7df8802cfdd,
        _:N458008bc6195484e9cc557f70eabda31 ;
    dct:created "2024-12-17"^^xsd:date ;
    dct:source "GDPR Art.14-5d"@en ;
    rdfs:isDefinedBy eu-gdpr: ;
    sw:term_status "accepted"@en ;
    skos:broader justifications:ConfidentialityObligationCompromised ;
    skos:definition "Justification that A14 obligations for providing information cannot be fulfilled as the personal data must remain confidential subject to an obligation of professional secrecy regulated by Union or Member State law, including a statutory obligation of secrecy"@en ;
    skos:inScheme eu-gdpr:rights-justifications-classes ;
    skos:prefLabel "Justification A14 - Confidentiality Compromised"@en ;
    skos:scopeNote "This justification requires information on which legal provision provides the confidentiality obligation, which can be provided as a description of comment, or ideally through dpv:hasApplicableLaw to refer to the specific law or through dpv:hasLegalBasis to refer to the specific legal basis enabling this justification"@en .

eu-gdpr:JustificationA14DisproportionateEffort a rdfs:Class,
        skos:Concept,
        dpv:Justification ;
    dct:contributor _:N05cd1f43dbaf4b4ba297dab5ee221394,
        _:N0a43dd9ea5e94fe695d8b7df8802cfdd,
        _:N458008bc6195484e9cc557f70eabda31 ;
    dct:created "2024-12-17"^^xsd:date ;
    dct:source "GDPR Art.14-5b"@en ;
    rdfs:isDefinedBy eu-gdpr: ;
    sw:term_status "accepted"@en ;
    skos:broader justifications:DisproportionateEffortRequired ;
    skos:definition "Justification that A14 obligations for providing information will require a disproportionate effort to fulfill"@en ;
    skos:inScheme eu-gdpr:rights-justifications-classes ;
    skos:prefLabel "Justification A14 - Disproportionate Effort"@en ;
    skos:scopeNote "This justification requires information on why the effort is considered disproportionate, such as the amount of time or resources required, which can be provided as a description of comment"@en .

eu-gdpr:JustificationA14EntityAlreadyInformed a rdfs:Class,
        skos:Concept,
        dpv:Justification ;
    dct:contributor _:N05cd1f43dbaf4b4ba297dab5ee221394,
        _:N0a43dd9ea5e94fe695d8b7df8802cfdd,
        _:N458008bc6195484e9cc557f70eabda31 ;
    dct:created "2024-12-17"^^xsd:date ;
    dct:source "GDPR Art.14-5a"@en ;
    rdfs:isDefinedBy eu-gdpr: ;
    sw:term_status "accepted"@en ;
    skos:broader justifications:EntityAlreadyInformed ;
    skos:definition "Justification that A14 obligations for providing information do not apply as the data subject already has the information"@en ;
    skos:inScheme eu-gdpr:rights-justifications-classes ;
    skos:prefLabel "Justification A14 - Entity Already Informed"@en ;
    skos:scopeNote "This justification requires information on how the data subject was provided the information to satify the assertion, which can be provided as a description of comment"@en .

eu-gdpr:JustificationA14FulfilmentImpossible a rdfs:Class,
        skos:Concept,
        dpv:Justification ;
    dct:contributor _:N05cd1f43dbaf4b4ba297dab5ee221394,
        _:N0a43dd9ea5e94fe695d8b7df8802cfdd,
        _:N458008bc6195484e9cc557f70eabda31 ;
    dct:created "2024-12-17"^^xsd:date ;
    dct:source "GDPR Art.14-5b"@en ;
    rdfs:isDefinedBy eu-gdpr: ;
    sw:term_status "accepted"@en ;
    skos:broader justifications:FulfilmentImpossible ;
    skos:definition "Justification that A14 obligations for providing information are impossible to fulfill"@en ;
    skos:inScheme eu-gdpr:rights-justifications-classes ;
    skos:prefLabel "Justification A14 - Fulfilment Impossible"@en ;
    skos:scopeNote "This justification requires information for why the fulfilment is impossible, such as technical impossibility, which can be provided as a description of comment"@en .

eu-gdpr:JustificationA14LegallyExempted a rdfs:Class,
        skos:Concept,
        dpv:Justification ;
    dct:contributor _:N05cd1f43dbaf4b4ba297dab5ee221394,
        _:N0a43dd9ea5e94fe695d8b7df8802cfdd,
        _:N458008bc6195484e9cc557f70eabda31 ;
    dct:created "2024-12-17"^^xsd:date ;
    dct:source "GDPR Art.14-5c"@en ;
    rdfs:isDefinedBy eu-gdpr: ;
    sw:term_status "accepted"@en ;
    skos:broader justifications:LegallyExempted ;
    skos:definition "Justification that A14 obligations for providing information is legally exempted"@en ;
    skos:inScheme eu-gdpr:rights-justifications-classes ;
    skos:prefLabel "Justification A14 - Legally Exempted"@en ;
    skos:scopeNote "This justification requires information on which legal provision provides the exemption, which can be provided as a description of comment, or ideally through dpv:hasApplicableLaw to refer to the specific law or through dpv:hasLegalBasis to refer to the specific legal basis enabling this justification"@en .

eu-gdpr:JustificationA14ObjectivesImpaired a rdfs:Class,
        skos:Concept,
        dpv:Justification ;
    dct:contributor _:N05cd1f43dbaf4b4ba297dab5ee221394,
        _:N0a43dd9ea5e94fe695d8b7df8802cfdd,
        _:N458008bc6195484e9cc557f70eabda31 ;
    dct:created "2024-12-17"^^xsd:date ;
    dct:source "GDPR Art.14-5b"@en ;
    rdfs:isDefinedBy eu-gdpr: ;
    sw:term_status "accepted"@en ;
    skos:broader justifications:ObjectivesImpaired ;
    skos:definition "Justification that A14 obligations for providing information will (seriously) impair the objectives of the processing"@en ;
    skos:inScheme eu-gdpr:rights-justifications-classes ;
    skos:prefLabel "Justification A14 - Objectives Impaired"@en ;
    skos:scopeNote "This justification requires information on what objectives are being impaired and the nature of impairment, which can be provided as a description of comment"@en .

eu-gdpr:JustificationA17Archiving a rdfs:Class,
        skos:Concept,
        dpv:Justification ;
    dct:contributor _:N0a43dd9ea5e94fe695d8b7df8802cfdd ;
    dct:created "2024-12-17"^^xsd:date ;
    dct:source "GDPR Art.17-"@en ;
    rdfs:isDefinedBy eu-gdpr: ;
    sw:term_status "accepted"@en ;
    skos:broader justifications:PublicInterestArchivingImpaired ;
    skos:definition "Justification that the A17 right to erasure or to be forgotten could not be completed due to"@en ;
    skos:inScheme eu-gdpr:rights-justifications-classes ;
    skos:prefLabel "Justification A17 - Archiving"@en .

eu-gdpr:JustificationA17ChildData a rdfs:Class,
        skos:Concept,
        dpv:Justification ;
    dct:contributor _:N0a43dd9ea5e94fe695d8b7df8802cfdd,
        _:N458008bc6195484e9cc557f70eabda31 ;
    dct:created "2024-12-17"^^xsd:date ;
    dct:source "GDPR Art.17-"@en ;
    rdfs:isDefinedBy eu-gdpr: ;
    sw:term_status "accepted"@en ;
    skos:broader justifications:InformationSocietyServicesOffer ;
    skos:definition "Justification that the A17 right to erasure or to be forgotten is being exercised as the personal data of a child have been collected for information society services referred to in A8(1)"@en ;
    skos:inScheme eu-gdpr:rights-justifications-classes ;
    skos:prefLabel "Justification A17 - Child Data"@en .

eu-gdpr:JustificationA17FreedomOfExpression a rdfs:Class,
        skos:Concept,
        dpv:Justification ;
    dct:contributor _:N0a43dd9ea5e94fe695d8b7df8802cfdd ;
    dct:created "2024-12-17"^^xsd:date ;
    dct:source "GDPR Art.17-"@en ;
    rdfs:isDefinedBy eu-gdpr: ;
    sw:term_status "accepted"@en ;
    skos:broader justifications:FreedomOfExpressionImpaired ;
    skos:definition "Justification that the A17 right to erasure or to be forgotten could not be completed as the processing is necessary for exercising the right of freedom of expression and information"@en ;
    skos:inScheme eu-gdpr:rights-justifications-classes ;
    skos:prefLabel "Justification A17 - Freedom Of Expression"@en .

eu-gdpr:JustificationA17LegalClaims a rdfs:Class,
        skos:Concept,
        dpv:Justification ;
    dct:contributor _:N0a43dd9ea5e94fe695d8b7df8802cfdd ;
    dct:created "2024-12-17"^^xsd:date ;
    dct:source "GDPR Art.17-"@en ;
    rdfs:isDefinedBy eu-gdpr: ;
    sw:term_status "accepted"@en ;
    skos:broader justifications:LegalClaimImpaired ;
    skos:definition "Justification that the A17 right to erasure or to be forgotten could not be completed due to"@en ;
    skos:inScheme eu-gdpr:rights-justifications-classes ;
    skos:prefLabel "Justification A17 - Legal Claims"@en .

eu-gdpr:JustificationA17LegalErasure a rdfs:Class,
        skos:Concept,
        dpv:Justification ;
    dct:contributor _:N0a43dd9ea5e94fe695d8b7df8802cfdd,
        _:N458008bc6195484e9cc557f70eabda31 ;
    dct:created "2024-12-17"^^xsd:date ;
    dct:source "GDPR Art.17-"@en ;
    rdfs:isDefinedBy eu-gdpr: ;
    sw:term_status "accepted"@en ;
    skos:broader justifications:LegalObligation ;
    skos:definition "Justification that the A17 right to erasure or to be forgotten is being exercised as the personal data have to be erased for compliance with a legal obligation in Union or Member State law to which the controller is subject"@en ;
    skos:inScheme eu-gdpr:rights-justifications-classes ;
    skos:prefLabel "Justification A17 - Legal Erasure"@en .

eu-gdpr:JustificationA17LegallyRequired a rdfs:Class,
        skos:Concept,
        dpv:Justification ;
    dct:contributor _:N0a43dd9ea5e94fe695d8b7df8802cfdd ;
    dct:created "2024-12-17"^^xsd:date ;
    dct:source "GDPR Art.17-"@en ;
    rdfs:isDefinedBy eu-gdpr: ;
    sw:term_status "accepted"@en ;
    skos:broader justifications:LegalObligationImpaired ;
    skos:definition "Justification that the A17 right to erasure or to be forgotten could not be completed as the processing is required for compliance with a legal obligation"@en ;
    skos:inScheme eu-gdpr:rights-justifications-classes ;
    skos:prefLabel "Justification A17 - Legally Required"@en .

eu-gdpr:JustificationA17NoLegalBasis a rdfs:Class,
        skos:Concept,
        dpv:Justification ;
    dct:contributor _:N0a43dd9ea5e94fe695d8b7df8802cfdd,
        _:N458008bc6195484e9cc557f70eabda31 ;
    dct:created "2024-12-17"^^xsd:date ;
    dct:source "GDPR Art.17-"@en ;
    rdfs:isDefinedBy eu-gdpr: ;
    sw:term_status "accepted"@en ;
    skos:broader justifications:LegalityLackingObjection ;
    skos:definition "Justification that the A17 right to erasure or to be forgotten is being exercised as the corresponding consent has been withdrawn and there is no other legal basis for the processing"@en ;
    skos:inScheme eu-gdpr:rights-justifications-classes ;
    skos:prefLabel "Justification A17 - No Legal Basis"@en .

eu-gdpr:JustificationA17NonNecessity a rdfs:Class,
        skos:Concept,
        dpv:Justification ;
    dct:contributor _:N0a43dd9ea5e94fe695d8b7df8802cfdd,
        _:N458008bc6195484e9cc557f70eabda31 ;
    dct:created "2024-12-17"^^xsd:date ;
    dct:source "GDPR Art.17-"@en ;
    rdfs:isDefinedBy eu-gdpr: ;
    sw:term_status "accepted"@en ;
    skos:broader justifications:NonNecessityObjection ;
    skos:definition "Justification that the A17 right to erasure or to be forgotten is being exercised as the personal data are no longer necessary in relation to the purposes for which they were collected or otherwise processed"@en ;
    skos:inScheme eu-gdpr:rights-justifications-classes ;
    skos:prefLabel "Justification A17 - Non-Necessity"@en .

eu-gdpr:JustificationA17ObjectA21 a rdfs:Class,
        skos:Concept,
        dpv:Justification ;
    dct:contributor _:N0a43dd9ea5e94fe695d8b7df8802cfdd,
        _:N458008bc6195484e9cc557f70eabda31 ;
    dct:created "2024-12-17"^^xsd:date ;
    dct:source "GDPR Art.17-"@en ;
    rdfs:isDefinedBy eu-gdpr: ;
    sw:term_status "accepted"@en ;
    skos:broader justifications:Objection ;
    skos:definition "Justification that the A17 right to erasure or to be forgotten is being exercised through A21 right to object where there are no overriding legitimate grounds for the processing (A21-1) or as an objection to direct marketing (A21-2)"@en ;
    skos:inScheme eu-gdpr:rights-justifications-classes ;
    skos:prefLabel "Justification A17 - Object A21"@en .

eu-gdpr:JustificationA17OfficialAuthority a rdfs:Class,
        skos:Concept,
        dpv:Justification ;
    dct:contributor _:N0a43dd9ea5e94fe695d8b7df8802cfdd ;
    dct:created "2024-12-17"^^xsd:date ;
    dct:source "GDPR Art.17-"@en ;
    rdfs:isDefinedBy eu-gdpr: ;
    sw:term_status "accepted"@en ;
    skos:broader justifications:OfficialAuthorityExerciseImpaired ;
    skos:definition "Justification that the A17 right to erasure or to be forgotten could not be completed due to"@en ;
    skos:inScheme eu-gdpr:rights-justifications-classes ;
    skos:prefLabel "Justification A17 - Official Authority"@en .

eu-gdpr:JustificationA17PublicHealth a rdfs:Class,
        skos:Concept,
        dpv:Justification ;
    dct:contributor _:N0a43dd9ea5e94fe695d8b7df8802cfdd ;
    dct:created "2024-12-17"^^xsd:date ;
    dct:source "GDPR Art.17-"@en ;
    rdfs:isDefinedBy eu-gdpr: ;
    sw:term_status "accepted"@en ;
    skos:broader justifications:PublicHealthCompromised ;
    skos:definition "Justification that the A17 right to erasure or to be forgotten could not be completed due to"@en ;
    skos:inScheme eu-gdpr:rights-justifications-classes ;
    skos:prefLabel "Justification A17 - Public Health"@en .

eu-gdpr:JustificationA17PublicInterest a rdfs:Class,
        skos:Concept,
        dpv:Justification ;
    dct:contributor _:N0a43dd9ea5e94fe695d8b7df8802cfdd ;
    dct:created "2024-12-17"^^xsd:date ;
    dct:source "GDPR Art.17-"@en ;
    rdfs:isDefinedBy eu-gdpr: ;
    sw:term_status "accepted"@en ;
    skos:broader justifications:PublicInterestCompromised ;
    skos:definition "Justification that the A17 right to erasure or to be forgotten could not be completed due to"@en ;
    skos:inScheme eu-gdpr:rights-justifications-classes ;
    skos:prefLabel "Justification A17 - Public Interest"@en .

eu-gdpr:JustificationA17UnlawfulProcessing a rdfs:Class,
        skos:Concept,
        dpv:Justification ;
    dct:contributor _:N0a43dd9ea5e94fe695d8b7df8802cfdd,
        _:N458008bc6195484e9cc557f70eabda31 ;
    dct:created "2024-12-17"^^xsd:date ;
    dct:source "GDPR Art.17-"@en ;
    rdfs:isDefinedBy eu-gdpr: ;
    sw:term_status "accepted"@en ;
    skos:broader justifications:UnlawfulActivityObjection ;
    skos:definition "Justification that the A17 right to erasure or to be forgotten is being exercised as the personal data have been unlawfully processed"@en ;
    skos:inScheme eu-gdpr:rights-justifications-classes ;
    skos:prefLabel "Justification A17 - Unlawful Processing"@en .

eu-gdpr:JustificationA33BreachedDataIneffective a rdfs:Class,
        skos:Concept,
        dpv:Justification ;
    dct:contributor _:N05cd1f43dbaf4b4ba297dab5ee221394,
        _:N0a43dd9ea5e94fe695d8b7df8802cfdd,
        _:N458008bc6195484e9cc557f70eabda31 ;
    dct:created "2024-12-17"^^xsd:date ;
    dct:source "GDPR Article33(3a)"@en ;
    rdfs:isDefinedBy eu-gdpr: ;
    sw:term_status "accepted"@en ;
    skos:broader justifications:ProcessSafeguarded,
        eu-gdpr:DataBreachJustification ;
    skos:definition "Justification that the personal data breach was not communicated to the data subject as the controller has implemented appropriate technical and organisational protection measures, and those measures were applied to the personal data affected by the personal data breach, in particular those that render the personal data unintelligible to any person who is not authorised to access it, such as encryption i.e. the breached data cannot be effectively used"@en ;
    skos:inScheme eu-gdpr:data-breach-classes ;
    skos:prefLabel "Justification A33 - Breached Data Ineffective"@en .

eu-gdpr:JustificationA33DisproportionateEffort a rdfs:Class,
        skos:Concept,
        dpv:Justification ;
    dct:contributor _:N05cd1f43dbaf4b4ba297dab5ee221394,
        _:N0a43dd9ea5e94fe695d8b7df8802cfdd,
        _:N458008bc6195484e9cc557f70eabda31 ;
    dct:created "2024-12-17"^^xsd:date ;
    dct:source "GDPR Article33(3c)"@en ;
    rdfs:isDefinedBy eu-gdpr: ;
    sw:term_status "accepted"@en ;
    skos:broader justifications:DisproportionateEffortRequired,
        eu-gdpr:DataBreachJustification ;
    skos:definition "Justification that the personal data breach was not communicated to the data subject as it would involve disproportionate effort, and that a public communication or similar measure whereby the data subjects are informed in an equally effective manner has been deployed"@en ;
    skos:inScheme eu-gdpr:data-breach-classes ;
    skos:prefLabel "Justification A33 - Disproportionate Effort"@en .

eu-gdpr:JustificationA33NotificationDelay a rdfs:Class,
        skos:Concept,
        dpv:Justification ;
    dct:contributor _:N05cd1f43dbaf4b4ba297dab5ee221394,
        _:N0a43dd9ea5e94fe695d8b7df8802cfdd,
        _:N458008bc6195484e9cc557f70eabda31 ;
    dct:created "2024-12-17"^^xsd:date ;
    dct:source "GDPR Article33(1)"@en ;
    rdfs:isDefinedBy eu-gdpr: ;
    sw:term_status "accepted"@en ;
    skos:broader justifications:DelayJustification,
        eu-gdpr:DataBreachJustification ;
    skos:definition "Justification for why the notification about personal data breach to the authority was not communicated within 72 hours after having become aware of it"@en ;
    skos:inScheme eu-gdpr:data-breach-classes ;
    skos:prefLabel "Justification A33 - Notification Delay"@en .

eu-gdpr:JustificationA33RiskMitigated a rdfs:Class,
        skos:Concept,
        dpv:Justification ;
    dct:contributor _:N05cd1f43dbaf4b4ba297dab5ee221394,
        _:N0a43dd9ea5e94fe695d8b7df8802cfdd,
        _:N458008bc6195484e9cc557f70eabda31 ;
    dct:created "2024-12-17"^^xsd:date ;
    dct:source "GDPR Article33(3b)"@en ;
    rdfs:isDefinedBy eu-gdpr: ;
    sw:term_status "accepted"@en ;
    skos:broader justifications:RiskMitigated,
        eu-gdpr:DataBreachJustification ;
    skos:definition "Justification that the personal data breach was not communicated to the data subject as the controller has taken subsequent measures which ensure that the high risk to the rights and freedoms of data subjects is no longer likely to materialise"@en ;
    skos:inScheme eu-gdpr:data-breach-classes ;
    skos:prefLabel "Justification A33 - Risk Mitigated"@en .

eu-gdpr:JustificationA33RiskUnlikely a rdfs:Class,
        skos:Concept,
        dpv:Justification ;
    dct:contributor _:N05cd1f43dbaf4b4ba297dab5ee221394,
        _:N0a43dd9ea5e94fe695d8b7df8802cfdd,
        _:N458008bc6195484e9cc557f70eabda31 ;
    dct:created "2024-12-17"^^xsd:date ;
    dct:source "GDPR Article33(1)"@en ;
    rdfs:isDefinedBy eu-gdpr: ;
    sw:term_status "accepted"@en ;
    skos:broader justifications:RightsFreedomsImpactUnlikely,
        eu-gdpr:DataBreachJustification ;
    skos:definition "Justification that the notification about personal data breach was not communicated to the authority as it is unlikely to result in a risk to the rights and freedoms of natural persons"@en ;
    skos:inScheme eu-gdpr:data-breach-classes ;
    skos:prefLabel "Justification A33 - Risk Unlikely"@en .

eu-gdpr:LawfulnessPrinciple a rdfs:Class,
        skos:Concept,
        dpv:OrganisationalMeasure ;
    dct:contributor _:N05cd1f43dbaf4b4ba297dab5ee221394 ;
    dct:created "2024-05-12"^^xsd:date ;
    dct:source "GDPR Art.5-1a"@en ;
    rdfs:isDefinedBy eu-gdpr: ;
    sw:term_status "accepted"@en ;
    skos:broader dpv:Principle ;
    skos:definition "Principle stating personal data must be processed processed in a lawful manner in relation to the data subject"@en ;
    skos:inScheme eu-gdpr:principles-classes ;
    skos:prefLabel "Lawfulness Principle"@en .

eu-gdpr:LeadSupervisoryAuthority a rdfs:Class,
        skos:Concept ;
    dct:contributor _:N05cd1f43dbaf4b4ba297dab5ee221394,
        _:N0a43dd9ea5e94fe695d8b7df8802cfdd ;
    dct:created "2024-02-14"^^xsd:date ;
    dct:source " Guidelines 3/2018 on the territorial scope of the GDPR (Article 3) Version 2.1"@en,
        "GDPR Art.56"@en ;
    rdfs:isDefinedBy eu-gdpr: ;
    rdfs:subClassOf eu-gdpr:DataProtectionAuthority ;
    sw:term_status "accepted"@en ;
    skos:broader eu-gdpr:DataProtectionAuthority ;
    skos:definition "Authority with the primary responsibility for dealing with a cross-border data processing activity"@en ;
    skos:inScheme eu-gdpr:entities-classes ;
    skos:prefLabel "Lead Supervisory Authority"@en .

eu-gdpr:LocalSupervisoryAuthority a rdfs:Class,
        skos:Concept ;
    dct:contributor _:N05cd1f43dbaf4b4ba297dab5ee221394,
        _:N0a43dd9ea5e94fe695d8b7df8802cfdd ;
    dct:created "2024-02-14"^^xsd:date ;
    dct:source " Guidelines 3/2018 on the territorial scope of the GDPR (Article 3) Version 2.1"@en,
        "GDPR Art.56"@en ;
    rdfs:isDefinedBy eu-gdpr: ;
    rdfs:subClassOf eu-gdpr:DataProtectionAuthority ;
    sw:term_status "accepted"@en ;
    skos:broader eu-gdpr:DataProtectionAuthority ;
    skos:definition "Authority associated with the main or local establishment of an organisation"@en ;
    skos:inScheme eu-gdpr:entities-classes ;
    skos:prefLabel "Local Supervisory Authority"@en .

eu-gdpr:MainEstablishment a rdfs:Class,
        skos:Concept ;
    dct:contributor _:N05cd1f43dbaf4b4ba297dab5ee221394,
        _:N0a43dd9ea5e94fe695d8b7df8802cfdd ;
    dct:created "2024-02-14"^^xsd:date ;
    dct:source " GDPR Art.56"@en,
        " Guidelines 3/2018 on the territorial scope of the GDPR (Article 3) Version 2.1"@en,
        "GDPR Art.4-16"@en ;
    rdfs:isDefinedBy eu-gdpr: ;
    rdfs:subClassOf eu-gdpr:Establishment ;
    sw:term_status "accepted"@en ;
    skos:broader eu-gdpr:Establishment ;
    skos:definition "Main Establishment' means as regards a controller with establishments in more than one Member State, the place of its central administration in the Union, unless the decisions on the purposes and means of the processing of personal data are taken in another establishment of the controller in the Union and the latter establishment has the power to have such decisions implemented, in which case the establishment having taken such decisions is to be considered to be the main establishment; as regards a processor with establishments in more than one Member State, the place of its central administration in the Union, or, if the processor has no central administration in the Union, the establishment of the processor in the Union where the main processing activities in the context of the activities of an establishment of the processor take place to the extent that the processor is subject to specific obligations under this Regulation;"@en ;
    skos:inScheme eu-gdpr:entities-classes ;
    skos:prefLabel "Main Establishment"@en .

eu-gdpr:PersonalData a rdfs:Class,
        skos:Concept,
        dpv:PersonalData ;
    dct:contributor _:N0a43dd9ea5e94fe695d8b7df8802cfdd ;
    dct:created "2024-12-17"^^xsd:date ;
    rdf:value "sc" ;
    rdfs:isDefinedBy eu-gdpr: ;
    sw:term_status "accepted"@en ;
    skos:broader dpv:PersonalData ;
    skos:definition "Personal Data' means any information relating to an identified or identifiable natural person (‘Data Subject’)"@en ;
    skos:inScheme eu-gdpr:misc-concepts-classes ;
    skos:prefLabel "Personal Data"@en .

eu-gdpr:Processing a rdfs:Class,
        skos:Concept,
        dpv:Processing ;
    dct:contributor _:N0a43dd9ea5e94fe695d8b7df8802cfdd ;
    dct:created "2024-12-17"^^xsd:date ;
    rdf:value "sc" ;
    rdfs:isDefinedBy eu-gdpr: ;
    sw:term_status "accepted"@en ;
    skos:broader dpv:Processing ;
    skos:definition "‘Processing’ means any operation or set of operations which is performed on personal data or on sets of personal data, whether or not by automated means, such as collection, recording, organisation, structuring, storage, adaptation or alteration, retrieval, consultation, use, disclosure by transmission, dissemination or otherwise making available, alignment or combination, restriction, erasure or destruction"@en ;
    skos:inScheme eu-gdpr:misc-concepts-classes ;
    skos:prefLabel "Processing"@en .

eu-gdpr:Processor a rdfs:Class,
        skos:Concept ;
    dct:contributor _:N0a43dd9ea5e94fe695d8b7df8802cfdd ;
    dct:created "2024-12-17"^^xsd:date ;
    dct:source "GDPR Art.4-8"@en ;
    rdfs:isDefinedBy eu-gdpr: ;
    rdfs:subClassOf dpv:DataProcessor ;
    sw:term_status "accepted"@en ;
    skos:broader dpv:DataProcessor ;
    skos:definition "‘Processor’ means a natural or legal person, public authority, agency or other body which processes personal data on behalf of the controller"@en ;
    skos:inScheme eu-gdpr:entities-classes ;
    skos:prefLabel "Processor"@en .

eu-gdpr:ProcessorBreachNotice a rdfs:Class,
        skos:Concept,
        eu-gdpr:DataBreachNotice ;
    dct:created "2024-05-19"^^xsd:date ;
    dct:source "GDPR Article 33"@en ;
    rdfs:isDefinedBy eu-gdpr: ;
    sw:term_status "accepted"@en ;
    skos:broader eu-gdpr:DataBreachNotice ;
    skos:definition "Notice regarding a data breach to the Processor"@en ;
    skos:inScheme eu-gdpr:data-breach-classes ;
    skos:prefLabel "Processor Breach Notice"@en .

eu-gdpr:ProcessorBreachNotificationNeeded a rdfs:Class,
        skos:Concept,
        eu-gdpr:DataBreachNoticeRequirement ;
    dct:created "2024-05-19"^^xsd:date ;
    dct:source "GDPR Article 33"@en ;
    rdfs:isDefinedBy eu-gdpr: ;
    sw:term_status "accepted"@en ;
    skos:broader eu-gdpr:DataBreachNoticeRequirement ;
    skos:definition "Data Breach notification to the Processor is required"@en ;
    skos:inScheme eu-gdpr:data-breach-classes ;
    skos:prefLabel "Processor Breach Notification Needed"@en .

eu-gdpr:Profiling a rdfs:Class,
        skos:Concept,
        dpv:Profiling ;
    dct:contributor _:N0a43dd9ea5e94fe695d8b7df8802cfdd ;
    dct:created "2024-12-17"^^xsd:date ;
    rdf:value "eu-gdpr:Processing" ;
    rdfs:isDefinedBy eu-gdpr: ;
    sw:term_status "accepted"@en ;
    skos:broader dpv:Profiling ;
    skos:definition "‘Profiling’ means any form of automated processing of personal data consisting of the use of personal data to evaluate certain personal aspects relating to a natural person, in particular to analyse or predict aspects concerning that natural person’s performance at work, economic situation, health, personal preferences, interests, reliability, behaviour, location or movements"@en ;
    skos:inScheme eu-gdpr:misc-concepts-classes ;
    skos:prefLabel "Profiling"@en .

eu-gdpr:Pseudonymisation a rdfs:Class,
        skos:Concept,
        dpv:Pseudonymisation ;
    dct:contributor _:N0a43dd9ea5e94fe695d8b7df8802cfdd ;
    dct:created "2024-12-17"^^xsd:date ;
    rdf:value "dpv:TechnicalMeasure" ;
    rdfs:isDefinedBy eu-gdpr: ;
    sw:term_status "accepted"@en ;
    skos:broader dpv:Pseudonymisation ;
    skos:definition "Pseudonymisation’ means the processing of personal data in such a manner that the personal data can no longer be attributed to a specific data subject without the use of additional information, provided that such additional information is kept separately and is subject to technical and organisational measures to ensure that the personal data are not attributed to an identified or identifiable natural person"@en ;
    skos:inScheme eu-gdpr:misc-concepts-classes ;
    skos:prefLabel "Pseudonymisation"@en .

eu-gdpr:PurposeLimitationPrinciple a rdfs:Class,
        skos:Concept,
        dpv:OrganisationalMeasure ;
    dct:contributor _:N05cd1f43dbaf4b4ba297dab5ee221394 ;
    dct:created "2024-05-12"^^xsd:date ;
    dct:source "GDPR Art.5-1b"@en ;
    rdfs:isDefinedBy eu-gdpr: ;
    sw:term_status "accepted"@en ;
    skos:broader dpv:Principle ;
    skos:definition "Principle stating personal data collected for specified, explicit and legitimate purposes and not further processed in a manner that is incompatible with those purposes; further processing for archiving purposes in the public interest, scientific or historical research purposes or statistical purposes shall, in accordance with Article 89(1), not be considered to be incompatible with the initial purposes"@en ;
    skos:inScheme eu-gdpr:principles-classes ;
    skos:prefLabel "Purpose Limitation Principle"@en .

eu-gdpr:Recipient a rdfs:Class,
        skos:Concept ;
    dct:contributor _:N0a43dd9ea5e94fe695d8b7df8802cfdd ;
    dct:created "2024-12-17"^^xsd:date ;
    dct:source "GDPR Art.4-9"@en ;
    rdfs:isDefinedBy eu-gdpr: ;
    rdfs:subClassOf dpv:Recipient ;
    sw:term_status "accepted"@en ;
    skos:broader dpv:Recipient ;
    skos:definition "‘Recipient’ means a natural or legal person, public authority, agency or another body, to which the personal data are disclosed, whether a third party or not"@en ;
    skos:inScheme eu-gdpr:entities-classes ;
    skos:prefLabel "Recipient"@en .

eu-gdpr:Representative a rdfs:Class,
        skos:Concept ;
    dct:contributor _:N0a43dd9ea5e94fe695d8b7df8802cfdd ;
    dct:created "2024-12-17"^^xsd:date ;
    dct:source "GDPR Art.4-17"@en ;
    rdfs:isDefinedBy eu-gdpr: ;
    rdfs:subClassOf dpv:Representative ;
    sw:term_status "accepted"@en ;
    skos:broader dpv:Representative ;
    skos:definition "Representative’ means a natural or legal person established in the Union who, designated by the controller or processor in writing pursuant to Article 27, represents the controller or processor with regard to their respective obligations under this Regulation"@en ;
    skos:inScheme eu-gdpr:entities-classes ;
    skos:prefLabel "Representative"@en .

eu-gdpr:RightsRecipientsNotice a rdfs:Class,
        skos:Concept,
        dpv:OrganisationalMeasure ;
    dct:contributor _:N05cd1f43dbaf4b4ba297dab5ee221394,
        _:N0a43dd9ea5e94fe695d8b7df8802cfdd,
        _:N458008bc6195484e9cc557f70eabda31 ;
    dct:created "2022-11-09"^^xsd:date ;
    rdfs:isDefinedBy eu-gdpr: ;
    sw:term_status "accepted"@en ;
    skos:broader dpv:RightFulfilmentNotice ;
    skos:definition "A Notice provided in fulfilment of GDPR's Art.19 regarding Recipients to whom a rights exercise has been communicated, such as regarding rectification (A.16) or erasure of personal data (A.17) or restriction of processing (A.18)"@en ;
    skos:inScheme eu-gdpr:rights-classes ;
    skos:prefLabel "Rights Recipients Notice"@en .

eu-gdpr:SARNotice a rdfs:Class,
        skos:Concept,
        dpv:OrganisationalMeasure ;
    dct:contributor _:N05cd1f43dbaf4b4ba297dab5ee221394,
        _:N0a43dd9ea5e94fe695d8b7df8802cfdd,
        _:N458008bc6195484e9cc557f70eabda31 ;
    dct:created "2022-11-09"^^xsd:date ;
    rdfs:isDefinedBy eu-gdpr: ;
    sw:term_status "accepted"@en ;
    skos:broader dpv:RightFulfilmentNotice ;
    skos:definition "A Notice provided in fulfilment of GDPR's Art.15 regarding information to be provided for Right of Access or Subject Access Request (SAR)"@en ;
    skos:inScheme eu-gdpr:rights-classes ;
    skos:prefLabel "SAR Notice"@en .

eu-gdpr:SCCByCommission a rdfs:Class,
        skos:Concept,
        dpv:OrganisationalMeasure ;
    dct:contributor _:N05cd1f43dbaf4b4ba297dab5ee221394,
        _:N0a43dd9ea5e94fe695d8b7df8802cfdd,
        _:N1aa8f48a4f3a40e6a438f71be918d3a1,
        _:Nd0960ac69a57403fb5db2455be10d160 ;
    dct:created "2021-09-22"^^xsd:date ;
    dct:source [ a schema:WebPage ;
            schema:name "GDPR Art.46-2c" ;
            schema:url "https://eur-lex.europa.eu/eli/reg/2016/679/art_46/par_2/pnt_c/oj" ] ;
    rdfs:isDefinedBy eu-gdpr: ;
    sw:term_status "accepted"@en ;
    skos:broader eu-gdpr:DataTransferTool,
        eu-gdpr:StandardContractualClauses ;
    skos:definition "Standard contractual clauses adopted by the Commission in accordance with the examination procedure referred to in GDPR Article 93(2)"@en ;
    skos:inScheme eu-gdpr:data-transfers-classes ;
    skos:prefLabel "SCCs adopted by Commission"@en .

eu-gdpr:SCCBySupervisoryAuthority a rdfs:Class,
        skos:Concept,
        dpv:OrganisationalMeasure ;
    dct:contributor _:N05cd1f43dbaf4b4ba297dab5ee221394,
        _:N0a43dd9ea5e94fe695d8b7df8802cfdd,
        _:N1aa8f48a4f3a40e6a438f71be918d3a1,
        _:Nd0960ac69a57403fb5db2455be10d160 ;
    dct:created "2021-09-22"^^xsd:date ;
    dct:source [ a schema:WebPage ;
            schema:name "GDPR Art.46-2d" ;
            schema:url "https://eur-lex.europa.eu/eli/reg/2016/679/art_46/par_2/pnt_d/oj" ] ;
    rdfs:isDefinedBy eu-gdpr: ;
    sw:term_status "accepted"@en ;
    skos:broader eu-gdpr:DataTransferTool,
        eu-gdpr:StandardContractualClauses ;
    skos:definition "Standard data protection clauses adopted by a supervisory authority and approved by the Commission pursuant to the examination procedure referred to in GDPR Article 93(2)"@en ;
    skos:inScheme eu-gdpr:data-transfers-classes ;
    skos:prefLabel "SCCs adopted by Supervisory Authority"@en .

eu-gdpr:SingleEstablishment a rdfs:Class,
        skos:Concept ;
    dct:contributor _:N05cd1f43dbaf4b4ba297dab5ee221394,
        _:N0a43dd9ea5e94fe695d8b7df8802cfdd ;
    dct:created "2024-02-14"^^xsd:date ;
    dct:source "GDPR Art.23"@en ;
    rdfs:isDefinedBy eu-gdpr: ;
    rdfs:subClassOf eu-gdpr:Establishment ;
    sw:term_status "accepted"@en ;
    skos:broader eu-gdpr:Establishment ;
    skos:definition "A legal entity that is established in only one Member State"@en ;
    skos:inScheme eu-gdpr:entities-classes ;
    skos:prefLabel "Single Establishment"@en .

eu-gdpr:StandardContractualClauses a rdfs:Class,
        skos:Concept,
        dpv:OrganisationalMeasure ;
    dct:contributor _:N05cd1f43dbaf4b4ba297dab5ee221394,
        _:N0a43dd9ea5e94fe695d8b7df8802cfdd,
        _:N1aa8f48a4f3a40e6a438f71be918d3a1,
        _:Nd0960ac69a57403fb5db2455be10d160 ;
    dct:created "2021-09-22"^^xsd:date ;
    dct:source [ a schema:WebPage ;
            schema:name "Implementing Decision on SCC for Data Transfers" ;
            schema:url "https://eur-lex.europa.eu/eli/dec_impl/2021/914/oj" ] ;
    rdfs:isDefinedBy eu-gdpr: ;
    sw:term_status "accepted"@en ;
    skos:broader dpv:Contract,
        eu-gdpr:DataTransferTool ;
    skos:definition "Standard Contractual Clauses (SCCs) are pre-approved clauses by the EU for ensuring appropriate data protection safeguards intended for data transfers from the EU to third countries"@en ;
    skos:inScheme eu-gdpr:data-transfers-classes ;
    skos:prefLabel "Standard Contractual Clauses (SCC)"@en .

eu-gdpr:StorageLimitationPrinciple a rdfs:Class,
        skos:Concept,
        dpv:OrganisationalMeasure ;
    dct:contributor _:N05cd1f43dbaf4b4ba297dab5ee221394 ;
    dct:created "2024-05-12"^^xsd:date ;
    dct:source "GDPR Art.5-1e"@en ;
    rdfs:isDefinedBy eu-gdpr: ;
    sw:term_status "accepted"@en ;
    skos:broader dpv:Principle ;
    skos:definition "Principle stating personal data must be kept in a form which permits identification of data subjects for no longer than is necessary for the purposes for which the personal data are processed; personal data may be stored for longer periods insofar as the personal data will be processed solely for archiving purposes in the public interest, scientific or historical research purposes or statistical purposes in accordance with Article 89(1) subject to implementation of the appropriate technical and organisational measures required by this Regulation in order to safeguard the rights and freedoms of the data subject"@en ;
    skos:inScheme eu-gdpr:principles-classes ;
    skos:prefLabel "Storage Limitation Principle"@en .

eu-gdpr:SupplementaryMeasure a rdfs:Class,
        skos:Concept,
        dpv:OrganisationalMeasure ;
    dct:contributor _:N05cd1f43dbaf4b4ba297dab5ee221394,
        _:N0a43dd9ea5e94fe695d8b7df8802cfdd,
        _:N1aa8f48a4f3a40e6a438f71be918d3a1 ;
    dct:created "2021-09-22"^^xsd:date ;
    dct:source [ a schema:WebPage ;
            schema:name "EDPB Recommendations 01/2020 on Supplementary Measures and Transfer Tools" ;
            schema:url "https://edpb.europa.eu/system/files/2021-06/edpb_recommendations_202001vo.2.0_supplementarymeasurestransferstools_en.pdf" ] ;
    rdfs:isDefinedBy eu-gdpr: ;
    sw:term_status "accepted"@en ;
    skos:broader eu-gdpr:DataTransferTool ;
    skos:definition "Supplementary measures are intended to additionally provide safeguards or guarantees to bring the resulting protection in line with EU requirements"@en ;
    skos:inScheme eu-gdpr:data-transfers-classes ;
    skos:prefLabel "Supplementary Measure"@en .

eu-gdpr:ThirdParty a rdfs:Class,
        skos:Concept ;
    dct:contributor _:N0a43dd9ea5e94fe695d8b7df8802cfdd ;
    dct:created "2024-12-17"^^xsd:date ;
    dct:source "GDPR Art.4-10"@en ;
    rdfs:isDefinedBy eu-gdpr: ;
    rdfs:subClassOf dpv:ThirdParty ;
    sw:term_status "accepted"@en ;
    skos:broader dpv:ThirdParty ;
    skos:definition "‘Third Party’ means a natural or legal person, public authority, agency or body other than the data subject, controller, processor and persons who, under the direct authority of the controller or processor, are authorised to process personal data"@en ;
    skos:inScheme eu-gdpr:entities-classes ;
    skos:prefLabel "Third Party"@en .

eu-gdpr:TransparencyPrinciple a rdfs:Class,
        skos:Concept,
        dpv:OrganisationalMeasure ;
    dct:contributor _:N05cd1f43dbaf4b4ba297dab5ee221394 ;
    dct:created "2024-05-12"^^xsd:date ;
    dct:source "GDPR Art.5-1a"@en ;
    rdfs:isDefinedBy eu-gdpr: ;
    sw:term_status "accepted"@en ;
    skos:broader dpv:Principle ;
    skos:definition "Principle stating personal data must be processed processed in a transparent manner in relation to the data subject"@en ;
    skos:inScheme eu-gdpr:principles-classes ;
    skos:prefLabel "Transparency Principle"@en .

dct:conformsTo a rdf:Property,
        skos:Concept ;
    rdfs:isDefinedBy eu-gdpr: ;
    skos:inScheme eu-gdpr:dpia-properties ;
    skos:prefLabel "dct:conformsTo"@en ;
    skos:scopeNote "For expressing an existing standard, guideline, or requirements to which the DPIA document or process will be conforming to. This could be external guidelines published by an Authority, or internal guidelines established by the organisation"@en .

dct:coverage a rdf:Property,
        skos:Concept ;
    rdfs:isDefinedBy eu-gdpr: ;
    skos:inScheme eu-gdpr:dpia-properties ;
    skos:prefLabel "dct:coverage"@en ;
    skos:scopeNote "For expressing coverage (e.g. jurisdictions, products, services) of the DPIA document or process. For temporal coverage, please see dct:temporal. The coverage can be expressed using dpv:Process, or using another concept, or even be a link or reference to a document, or a textual description"@en .

dct:created a rdf:Property,
        skos:Concept ;
    rdfs:isDefinedBy eu-gdpr: ;
    skos:inScheme eu-gdpr:dpia-properties ;
    skos:prefLabel "dct:created"@en ;
    skos:scopeNote "For expressing when the documentation (e.g. DPIA Necessity Assessment, or DPIA Procedure, or DPIA outcome) was created"@en .

dct:dateAccepted a rdf:Property,
        skos:Concept ;
    rdfs:isDefinedBy eu-gdpr: ;
    skos:inScheme eu-gdpr:dpia-properties ;
    skos:prefLabel "dct:dateAccepted"@en ;
    skos:scopeNote "For expressing when the documentation (e.g. DPIA Necessity Assessment, or DPIA Procedure, or DPIA outcome) was accepted through audit or approval"@en .

dct:dateSubmitted a rdf:Property,
        skos:Concept ;
    rdfs:isDefinedBy eu-gdpr: ;
    skos:inScheme eu-gdpr:dpia-properties ;
    skos:prefLabel "dct:dateSubmitted"@en ;
    skos:scopeNote "For expressing when the documentation (e.g. DPIA Necessity Assessment, or DPIA Procedure, or DPIA outcome) was submitted for audit or approval"@en .

dct:description a rdf:Property,
        skos:Concept ;
    rdfs:isDefinedBy eu-gdpr: ;
    skos:inScheme eu-gdpr:dpia-properties ;
    skos:prefLabel "dct:description"@en ;
    skos:scopeNote "Indicates a description of the DPIA for human comprehension"@en .

dct:hasPart a rdf:Property,
        skos:Concept ;
    rdfs:isDefinedBy eu-gdpr: ;
    skos:inScheme eu-gdpr:dpia-properties ;
    skos:prefLabel "dct:hasPart"@en ;
    skos:scopeNote "For expressing something contains a DPIA document or process contains as a part. For example, as some dpv:DPIA dct:hasPart DPIANecessityAssessment"@en .

dct:identifier a rdf:Property,
        skos:Concept ;
    rdfs:isDefinedBy eu-gdpr: ;
    skos:inScheme eu-gdpr:dpia-properties ;
    skos:prefLabel "dct:identifier"@en ;
    skos:scopeNote "Indicates an identifier associated with the DPIA documentation or process. Identifiers may be reused from existing systems, or created for the purposes of record management"@en .

dct:isPartOf a rdf:Property,
        skos:Concept ;
    rdfs:isDefinedBy eu-gdpr: ;
    skos:inScheme eu-gdpr:dpia-properties ;
    skos:prefLabel "dct:isPartOf"@en ;
    skos:scopeNote "For expressing a DPIA document or process is part of another. For example, as some DPIANecessityAssessment dct:isPartOf some dpv:DPIA"@en .

dct:isVersionOf a rdf:Property,
        skos:Concept ;
    rdfs:isDefinedBy eu-gdpr: ;
    skos:inScheme eu-gdpr:dpia-properties ;
    skos:prefLabel "dct:isVersionOf"@en ;
    skos:scopeNote "For expressing prior versions or iterations of the DPIA document or process"@en .

dct:modified a rdf:Property,
        skos:Concept ;
    rdfs:isDefinedBy eu-gdpr: ;
    skos:inScheme eu-gdpr:dpia-properties ;
    skos:prefLabel "dct:modified"@en ;
    skos:scopeNote "For expressing when the documentation (e.g. DPIA Necessity Assessment, or DPIA Procedure, or DPIA outcome) was last modified"@en .

dct:subject a rdf:Property,
        skos:Concept ;
    rdfs:isDefinedBy eu-gdpr: ;
    skos:inScheme eu-gdpr:dpia-properties ;
    skos:prefLabel "dct:subject"@en ;
    skos:scopeNote "For expressing the subject of the DPIA document or process, where subject refers to the point of focus. For expressing what is affected or included within the DPIA, please see dct:coverage"@en .

dct:temporal a rdf:Property,
        skos:Concept ;
    rdfs:isDefinedBy eu-gdpr: ;
    skos:inScheme eu-gdpr:dpia-properties ;
    skos:prefLabel "dct:temporal"@en ;
    skos:scopeNote "For expressing the temporal coverage of the DPIA document or process"@en .

dct:title a rdf:Property,
        skos:Concept ;
    rdfs:isDefinedBy eu-gdpr: ;
    skos:inScheme eu-gdpr:dpia-properties ;
    skos:prefLabel "dct:title"@en ;
    skos:scopeNote "Indicates a title of the DPIA for human comprehension"@en .

dct:valid a rdf:Property,
        skos:Concept ;
    rdfs:isDefinedBy eu-gdpr: ;
    skos:inScheme eu-gdpr:dpia-properties ;
    skos:prefLabel "dct:valid"@en ;
    skos:scopeNote "For expressing the temporal date or range of validity of the DPIA document or process. This refers to the time period for which the DPIA is considered valid, and does not refer to the temporal period associated with processing (see dct:temporal instead). The assumption is that after this period, the DPIA should be re-evaluated or some process should be triggered"@en .

dpv:hasStatus a rdf:Property,
        skos:Concept ;
    vann:example dex:E0069 ;
    rdfs:isDefinedBy eu-gdpr: ;
    skos:inScheme eu-gdpr:dpia-properties ;
    skos:scopeNote "For expressing the status of the DPIA document or process. Here different statuses are used to convey different contextual meanings. For example, dpv:ActivityStatus expresses the state of the activity in terms of whether it is ongoing or completed, and dpv:AuditStatus expresses the state of the audit process in terms of being required, approved, or rejected. These are applied over each step of the DPIA i.e. DPIANecessityAssessment, DPIAProcedure, and DPIAOutcome. Similarly, a process also uses hasStatus with DPIAConformity to indicate adherence to the results of the DPIA process."@en .

<https://w3id.org/dpv/legal/eu/gdpr> a owl:Ontology,
        profile:Profile ;
    dct:bibliographicCitation "Harshvardhan J. Pandit, Beatriz Esteves, Georg P. Krog, Paul Ryan, Delaram Golpayegani, Julian Flake (2025) Data Privacy Vocabulary (DPV) – Version 2.0. In: Demartini, G., et al. The Semantic Web – ISWC 2024. ISWC 2024. Lecture Notes in Computer Science, vol 15233. Springer, Cham. https://doi.org/10.1007/978-3-031-77847-6_10" ;
    dct:conformsTo "http://www.w3.org/2000/01/rdf-schema",
        "http://www.w3.org/2004/02/skos/core" ;
    dct:contributor _:N05cd1f43dbaf4b4ba297dab5ee221394,
        _:N0a43dd9ea5e94fe695d8b7df8802cfdd,
        _:N1aa8f48a4f3a40e6a438f71be918d3a1,
        _:N2b1e6adbca7e4e73a4c12246fc8d2f06,
        _:N458008bc6195484e9cc557f70eabda31,
        _:N6bd5cc92354a4f6e91cef68caab7fcdd,
        _:Nd0960ac69a57403fb5db2455be10d160,
        _:Nd401626ea33444c4a84dfef86e49d9f5 ;
    dct:created "2019-06-18"@en ;
    dct:creator _:N05cd1f43dbaf4b4ba297dab5ee221394,
        _:N0a43dd9ea5e94fe695d8b7df8802cfdd,
        _:N458008bc6195484e9cc557f70eabda31,
        _:Nd0960ac69a57403fb5db2455be10d160 ;
    dct:description "Extension to the Data Privacy Vocabulary (DPV) providing concepts for representing information associated with EU GDPR"@en ;
    dct:identifier "https://w3id.org/dpv/legal/eu/gdpr" ;
    dct:issued "2019-06-18"@en ;
    dct:license <https://www.w3.org/copyright/document-license-2023/> ;
    dct:modified "2025-03-16"@en ;
    dct:publisher <https://www.w3.org/> ;
    dct:source <https://www.w3.org/groups/cg/dpvcg/> ;
    dct:title "EU General Data Protection Regulation (GDPR)"@en ;
    bibo:doi "10.5281/zenodo.12505841" ;
    bibo:status "http://purl.org/ontology/bibo/status/published" ;
    vann:preferredNamespacePrefix "eu-gdpr" ;
    vann:preferredNamespaceUri "https://w3id.org/dpv/legal/eu/gdpr#" ;
    rdfs:Label "EU-GDPR"@en ;
    owl:versionIRI <https://w3id.org/dpv/2.1/legal/eu/gdpr> ;
    owl:versionInfo "2.1" ;
    profile:hasResource <https://w3id.org/dpv/examples>,
        <https://w3id.org/dpv/guides>,
        eu-gdpr:serialisation-html,
        eu-gdpr:serialisation-jsonld,
        eu-gdpr:serialisation-n3,
        eu-gdpr:serialisation-rdf,
        eu-gdpr:serialisation-ttl,
        <https://w3id.org/dpv/primer> ;
    profile:isProfileOf rdfs:,
        skos:,
        <https://w3id.org/dpv> ;
    foaf:logo <https://w3id.org/dpv/media/logo.png> ;
    schema:version "2.1" .

eu-gdpr:A6-1-d-natual-person dpv:hasRight eu-gdpr:A13,
        eu-gdpr:A14,
        eu-gdpr:A15,
        eu-gdpr:A16,
        eu-gdpr:A17,
        eu-gdpr:A18,
        eu-gdpr:A22,
        eu-gdpr:A77 .

eu-gdpr:hasConcernedSA a rdf:Property,
        skos:Concept ;
    dcam:rangeIncludes dpv:DataProtectionAuthority ;
    dct:contributor _:N05cd1f43dbaf4b4ba297dab5ee221394,
        _:N0a43dd9ea5e94fe695d8b7df8802cfdd ;
    dct:created "2024-02-14"^^xsd:date ;
    dct:source " Guidelines 3/2018 on the territorial scope of the GDPR (Article 3) Version 2.1"@en,
        "GDPR Art.56"@en ;
    rdfs:isDefinedBy eu-gdpr: ;
    rdfs:subPropertyOf dpv:hasEntity ;
    sw:term_status "accepted"@en ;
    skos:broader dpv:hasEntity ;
    skos:definition "Indicates a concerned supervisory authority"@en ;
    skos:inScheme eu-gdpr:entities-properties ;
    skos:prefLabel "has concerned supervisory authority"@en ;
    schema:rangeIncludes dpv:DataProtectionAuthority .

eu-gdpr:hasEstablishment a rdf:Property,
        skos:Concept ;
    dcam:domainIncludes dpv:LegalEntity ;
    dcam:rangeIncludes dpv:LegalEntity ;
    dct:contributor _:N05cd1f43dbaf4b4ba297dab5ee221394,
        _:N0a43dd9ea5e94fe695d8b7df8802cfdd ;
    dct:created "2024-02-14"^^xsd:date ;
    dct:source " Guidelines 3/2018 on the territorial scope of the GDPR (Article 3) Version 2.1"@en,
        "GDPR Art.56"@en ;
    rdfs:isDefinedBy eu-gdpr: ;
    rdfs:subPropertyOf dpv:hasEntity ;
    sw:term_status "accepted"@en ;
    skos:broader dpv:hasEntity ;
    skos:definition "Indicates an establishment associated with a legal entity"@en ;
    skos:inScheme eu-gdpr:entities-properties ;
    skos:prefLabel "has establishment"@en ;
    schema:domainIncludes dpv:LegalEntity ;
    schema:rangeIncludes dpv:LegalEntity .

eu-gdpr:hasLeadSA a rdf:Property,
        skos:Concept ;
    dcam:rangeIncludes dpv:DataProtectionAuthority ;
    dct:contributor _:N05cd1f43dbaf4b4ba297dab5ee221394,
        _:N0a43dd9ea5e94fe695d8b7df8802cfdd ;
    dct:created "2024-02-14"^^xsd:date ;
    dct:source " Guidelines 3/2018 on the territorial scope of the GDPR (Article 3) Version 2.1"@en,
        "GDPR Art.56"@en ;
    rdfs:isDefinedBy eu-gdpr: ;
    rdfs:subPropertyOf dpv:hasEntity ;
    sw:term_status "accepted"@en ;
    skos:broader dpv:hasEntity ;
    skos:definition "Indicates the lead supervisory authority"@en ;
    skos:inScheme eu-gdpr:entities-properties ;
    skos:prefLabel "has lead supervisory authority"@en ;
    schema:rangeIncludes dpv:DataProtectionAuthority .

eu-gdpr:hasLocalSA a rdf:Property,
        skos:Concept ;
    dcam:rangeIncludes dpv:DataProtectionAuthority ;
    dct:contributor _:N05cd1f43dbaf4b4ba297dab5ee221394,
        _:N0a43dd9ea5e94fe695d8b7df8802cfdd ;
    dct:created "2024-02-14"^^xsd:date ;
    dct:source " Guidelines 3/2018 on the territorial scope of the GDPR (Article 3) Version 2.1"@en,
        "GDPR Art.56"@en ;
    rdfs:isDefinedBy eu-gdpr: ;
    rdfs:subPropertyOf dpv:hasEntity ;
    sw:term_status "accepted"@en ;
    skos:broader dpv:hasEntity ;
    skos:definition "Indicates the local supervisory authority"@en ;
    skos:inScheme eu-gdpr:entities-properties ;
    skos:prefLabel "has local supervisory authority"@en ;
    schema:rangeIncludes dpv:DataProtectionAuthority .

eu-gdpr:hasMainEstablishment a rdf:Property,
        skos:Concept ;
    dcam:domainIncludes dpv:LegalEntity ;
    dcam:rangeIncludes dpv:LegalEntity ;
    dct:contributor _:N05cd1f43dbaf4b4ba297dab5ee221394,
        _:N0a43dd9ea5e94fe695d8b7df8802cfdd ;
    dct:created "2024-02-14"^^xsd:date ;
    dct:source " Guidelines 3/2018 on the territorial scope of the GDPR (Article 3) Version 2.1"@en,
        "GDPR Art.56"@en ;
    rdfs:isDefinedBy eu-gdpr: ;
    rdfs:subPropertyOf dpv:hasEntity ;
    sw:term_status "accepted"@en ;
    skos:broader dpv:hasEntity ;
    skos:definition "Indicates the legal entity has specified establishment as its main establishment"@en ;
    skos:inScheme eu-gdpr:entities-properties ;
    skos:prefLabel "has main establishment"@en ;
    schema:domainIncludes dpv:LegalEntity ;
    schema:rangeIncludes dpv:LegalEntity .

eu-gdpr:isMainEstablishmentFor a rdf:Property,
        skos:Concept ;
    dcam:domainIncludes dpv:LegalEntity ;
    dcam:rangeIncludes dpv:LegalEntity ;
    dct:contributor _:N05cd1f43dbaf4b4ba297dab5ee221394,
        _:N0a43dd9ea5e94fe695d8b7df8802cfdd ;
    dct:created "2024-02-14"^^xsd:date ;
    dct:source " Guidelines 3/2018 on the territorial scope of the GDPR (Article 3) Version 2.1"@en,
        "GDPR Art.56"@en ;
    rdfs:isDefinedBy eu-gdpr: ;
    rdfs:subPropertyOf dpv:hasEntity ;
    sw:term_status "accepted"@en ;
    skos:broader dpv:hasEntity ;
    skos:definition "Indicates the main establishment for specific legal entity"@en ;
    skos:inScheme eu-gdpr:entities-properties ;
    skos:prefLabel "is main establishment for"@en ;
    schema:domainIncludes dpv:LegalEntity ;
    schema:rangeIncludes dpv:LegalEntity .

eu-gdpr:serialisation-html a profile:ResourceDescriptor ;
    dct:conformsTo <https://www.w3.org/TR/html/> ;
    dct:format <https://www.iana.org/assignments/media-types/text/html> ;
    dct:title "EU General Data Protection Regulation (GDPR) - HTML serialiation" ;
    profile:hasArtifact <https://w3id.org/dpv/legal/eu/gdpr/eu-gdpr.html> ;
    profile:hasRole role:specification .

eu-gdpr:serialisation-jsonld a profile:ResourceDescriptor ;
    dct:conformsTo <https://www.w3.org/TR/json-ld11/> ;
    dct:format <https://www.iana.org/assignments/media-types/application/ld+json> ;
    dct:title "EU General Data Protection Regulation (GDPR) - JSON-LD serialiation" ;
    profile:hasArtifact <https://w3id.org/dpv/legal/eu/gdpr/eu-gdpr.jsonld> ;
    profile:hasRole role:vocabulary .

eu-gdpr:serialisation-n3 a profile:ResourceDescriptor ;
    dct:conformsTo <https://www.w3.org/TeamSubmission/n3/> ;
    dct:format <https://www.iana.org/assignments/media-types/text/n3> ;
    dct:title "EU General Data Protection Regulation (GDPR) - N3 serialiation" ;
    profile:hasArtifact <https://w3id.org/dpv/legal/eu/gdpr/eu-gdpr.n3> ;
    profile:hasRole role:vocabulary .

eu-gdpr:serialisation-rdf a profile:ResourceDescriptor ;
    dct:conformsTo rdf: ;
    dct:format <https://www.iana.org/assignments/media-types/application/rdf+xml> ;
    dct:title "EU General Data Protection Regulation (GDPR) - RDF/XML serialiation" ;
    profile:hasArtifact <https://w3id.org/dpv/legal/eu/gdpr/eu-gdpr.rdf> ;
    profile:hasRole role:vocabulary .

eu-gdpr:serialisation-ttl a profile:ResourceDescriptor ;
    dct:conformsTo <https://www.w3.org/TR/turtle/> ;
    dct:format <https://www.iana.org/assignments/media-types/text/turtle> ;
    dct:title "EU General Data Protection Regulation (GDPR) - Turtle serialiation" ;
    profile:hasArtifact <https://w3id.org/dpv/legal/eu/gdpr/eu-gdpr.ttl> ;
    profile:hasRole role:vocabulary .

<https://w3id.org/dpv/examples> a profile:ResourceDescriptor ;
    dct:conformsTo <https://www.w3.org/TR/html/> ;
    dct:format <https://www.iana.org/assignments/media-types/text/html> ;
    dct:title "Examples for Data Privacy Vocabulary" ;
    profile:hasArtifact <https://w3id.org/dpv/examples> ;
    profile:hasRole role:guidance .

<https://w3id.org/dpv/guides> a profile:ResourceDescriptor ;
    dct:conformsTo <https://www.w3.org/TR/html/> ;
    dct:format <https://www.iana.org/assignments/media-types/text/html> ;
    dct:title "Guides for Data Privacy Vocabulary" ;
    profile:hasArtifact <https://w3id.org/dpv/guides> ;
    profile:hasRole role:guidance .

<https://w3id.org/dpv/primer> a profile:ResourceDescriptor ;
    dct:conformsTo <https://www.w3.org/TR/html/> ;
    dct:format <https://www.iana.org/assignments/media-types/text/html> ;
    dct:title "Primer for Data Privacy Vocabulary" ;
    profile:hasArtifact <https://w3id.org/dpv/primer> ;
    profile:hasRole role:guidance .

eu-gdpr:compliance-classes a skos:ConceptScheme .

eu-gdpr:entities-properties a skos:ConceptScheme .

eu-gdpr:data-transfers-classes a skos:ConceptScheme .

eu-gdpr:misc-concepts-classes a skos:ConceptScheme .

eu-gdpr:principles-classes a skos:ConceptScheme .

eu-gdpr:legal-basis-special-classes a skos:ConceptScheme .

eu-gdpr:entities-classes a skos:ConceptScheme .

eu-gdpr:dpia-properties a skos:ConceptScheme .

eu-gdpr:legal-basis-classes a skos:ConceptScheme .

eu-gdpr:legal-basis-data-transfer-classes a skos:ConceptScheme .

eu-gdpr:rights-impacts-classes a skos:ConceptScheme .

eu-gdpr:dpia-classes a skos:ConceptScheme .

eu-gdpr:rights-classes a skos:ConceptScheme .

eu-gdpr:rights-justifications-classes a skos:ConceptScheme .

eu-gdpr:data-breach-classes a skos:ConceptScheme .

_:N011c6bcf62fd4c2192fb3efde478fd38 a foaf:Organization ;
    foaf:name "Unabhängige Landeszentrum für Datenschutz Schleswig-Holstein" .

_:N2bfb2dfcc0b24c5182bd06c242c085fa a foaf:Organization ;
    foaf:name "Signatu AS" .

_:N313d89a6c37147bfac1bbb4aa7f6510b a foaf:Organization ;
    foaf:name "ADAPT Centre, Dublin City University" .

_:N3f64d3533a104953b63bb217ff4665c5 a foaf:Organization ;
    foaf:name "IDLab, IMEC, Ghent University" .

_:N77a9e87e7f0e42959387d0b6a299325f a foaf:Organization ;
    foaf:name "Uniphar PLC" .

_:Nac2d5a6ba12d43d387d630afd6a760ea a foaf:Organization ;
    foaf:name "Dublin City University" .

_:Nb76f26fd1e4a404eba6614ee773e6fdf a foaf:Organization ;
    foaf:name "W3C/ERCIM" .

_:Nd52b364fe0b9434d864d3540772fca23 a foaf:Organization ;
    foaf:name "Unabhängige Landeszentrum für Datenschutz Schleswig-Holstein" .

_:Nd401626ea33444c4a84dfef86e49d9f5 a dct:Agent,
        foaf:Person ;
    org:memberOf _:Nb76f26fd1e4a404eba6614ee773e6fdf ;
    foaf:name "Rigo Wenning" .

_:Nd0960ac69a57403fb5db2455be10d160 a dct:Agent,
        foaf:Person ;
    scoro:hasORCID "0000-0003-0770-2737" ;
    org:memberOf _:N77a9e87e7f0e42959387d0b6a299325f ;
    foaf:name "Paul Ryan" .

_:N1aa8f48a4f3a40e6a438f71be918d3a1 a dct:Agent,
        foaf:Person ;
    org:memberOf _:Nac2d5a6ba12d43d387d630afd6a760ea ;
    foaf:name "David Hickey" .

_:N2b1e6adbca7e4e73a4c12246fc8d2f06 a dct:Agent,
        foaf:Person ;
    org:memberOf _:Nd52b364fe0b9434d864d3540772fca23 ;
    foaf:name "Bud Bruegger" .

_:N6bd5cc92354a4f6e91cef68caab7fcdd a dct:Agent,
        foaf:Person ;
    org:memberOf _:N011c6bcf62fd4c2192fb3efde478fd38 ;
    foaf:name "Eva Schlehahn" .

_:N458008bc6195484e9cc557f70eabda31 a dct:Agent,
        foaf:Person ;
    scoro:hasORCID "0000-0003-0259-7560" ;
    org:memberOf _:N3f64d3533a104953b63bb217ff4665c5 ;
    foaf:name "Beatriz Esteves" .

_:N05cd1f43dbaf4b4ba297dab5ee221394 a dct:Agent,
        foaf:Person ;
    org:memberOf _:N2bfb2dfcc0b24c5182bd06c242c085fa ;
    foaf:homepage "https://www.linkedin.com/in/georg-philip-krog-a2a278104/" ;
    foaf:name "Georg P. Krog" .

_:N0a43dd9ea5e94fe695d8b7df8802cfdd a dct:Agent,
        foaf:Person ;
    scoro:hasORCID "0000-0002-5068-3714" ;
    org:memberOf _:N313d89a6c37147bfac1bbb4aa7f6510b ;
    foaf:homepage "https://harshp.com/" ;
    foaf:name "Harshvardhan J. Pandit" .

