@prefix ai-owl: <https://w3id.org/dpv/ai/owl#> .
@prefix bibo: <http://purl.org/ontology/bibo/> .
@prefix dct: <http://purl.org/dc/terms/> .
@prefix dpv-owl: <https://w3id.org/dpv/owl#> .
@prefix foaf: <http://xmlns.com/foaf/0.1/> .
@prefix org: <http://www.w3.org/ns/org#> .
@prefix owl: <http://www.w3.org/2002/07/owl#> .
@prefix profile: <http://www.w3.org/ns/dx/prof/> .
@prefix rdf: <http://www.w3.org/1999/02/22-rdf-syntax-ns#> .
@prefix rdfs: <http://www.w3.org/2000/01/rdf-schema#> .
@prefix role: <http://www.w3.org/ns/dx/prof/role/> .
@prefix schema: <https://schema.org/> .
@prefix scoro: <http://purl.org/spar/scoro/> .
@prefix skos: <http://www.w3.org/2004/02/skos/core#> .
@prefix sw: <http://www.w3.org/2003/06/sw-vocab-status/ns#> .
@prefix vann: <http://purl.org/vocab/vann/> .
@prefix xsd: <http://www.w3.org/2001/XMLSchema#> .

ai-owl:ActionRecognition a rdfs:Class,
        owl:Class,
        ai-owl:Capability ;
    dct:contributor _:person-delaram-golpayegani ;
    dct:created "2024-12-01"^^xsd:date ;
    dct:source " Defining Artificial Intelligence 2.0"@en,
        "AI Watch"@en ;
    rdfs:isDefinedBy ai-owl: ;
    rdfs:subClassOf ai-owl:BiometricCapability,
        ai-owl:ComputerVision ;
    sw:term_status "accepted"@en ;
    skos:definition "Capability to recognise actions"@en ;
    skos:prefLabel "Action Recognition"@en .

ai-owl:AudioCapability a rdfs:Class,
        owl:Class,
        ai-owl:Capability ;
    dct:contributor _:person-harshvardhan-j-pandit ;
    dct:created "2024-12-01"^^xsd:date ;
    rdfs:isDefinedBy ai-owl: ;
    rdfs:subClassOf ai-owl:Capability ;
    sw:term_status "accepted"@en ;
    skos:definition "Capabilities related to the processing and generation of audio"@en ;
    skos:prefLabel "Audio Capability"@en .

ai-owl:AudioGeneration a rdfs:Class,
        owl:Class,
        ai-owl:Capability ;
    dct:contributor _:person-delaram-golpayegani,
        _:person-harshvardhan-j-pandit ;
    dct:created "2024-12-01"^^xsd:date ;
    rdfs:isDefinedBy ai-owl: ;
    rdfs:subClassOf ai-owl:AudioCapability,
        ai-owl:ContentGeneration ;
    sw:term_status "accepted"@en ;
    skos:definition "Capability to generate audio"@en ;
    skos:prefLabel "Audio Generation"@en .

ai-owl:AutomaticSummarisation a rdfs:Class,
        owl:Class,
        ai-owl:Capability ;
    dct:contributor _:person-delaram-golpayegani ;
    dct:created "2024-12-01"^^xsd:date ;
    dct:source "ISO/IEC 22989:2022 3.6.1"@en ;
    rdfs:isDefinedBy ai-owl: ;
    rdfs:subClassOf ai-owl:InformationRetrieval,
        ai-owl:LanguageCapability ;
    sw:term_status "accepted"@en ;
    skos:definition "Capability for shortening a portion of content such as text while retaining important semantic information"@en ;
    skos:prefLabel "Automatic Summarisation"@en .

ai-owl:BehaviourAnalysis a rdfs:Class,
        owl:Class,
        ai-owl:Capability ;
    dct:contributor _:person-delaram-golpayegani ;
    dct:created "2024-12-01"^^xsd:date ;
    rdfs:isDefinedBy ai-owl: ;
    rdfs:subClassOf ai-owl:HumanOrientedCapability ;
    sw:term_status "accepted"@en ;
    skos:definition "Capability of a system in analysing people's behaviour"@en ;
    skos:prefLabel "Behaviour Analysis"@en .

ai-owl:BiometricCapability a rdfs:Class,
        owl:Class,
        ai-owl:Capability ;
    dct:contributor _:person-delaram-golpayegani ;
    dct:created "2024-12-01"^^xsd:date ;
    rdfs:isDefinedBy ai-owl: ;
    rdfs:subClassOf ai-owl:HumanOrientedCapability ;
    sw:term_status "accepted"@en ;
    skos:definition "Capability involving processing of biometric data or related to biometrics"@en ;
    skos:prefLabel "Biometric Capability"@en .

ai-owl:BiometricCategorisation a rdfs:Class,
        owl:Class,
        ai-owl:Capability ;
    dct:contributor _:person-delaram-golpayegani ;
    dct:created "2024-12-01"^^xsd:date ;
    rdfs:isDefinedBy ai-owl: ;
    rdfs:subClassOf ai-owl:BiometricCapability ;
    sw:term_status "accepted"@en ;
    skos:definition "Capability involving assigning natural persons to specific categories based on their biometric data"@en ;
    skos:prefLabel "Biometric Categorisation"@en .

ai-owl:BiometricEmotionRecognition a rdfs:Class,
        owl:Class,
        ai-owl:Capability ;
    dct:contributor _:person-delaram-golpayegani ;
    dct:created "2024-12-01"^^xsd:date ;
    rdfs:isDefinedBy ai-owl: ;
    rdfs:subClassOf ai-owl:EmotionRecognition ;
    sw:term_status "accepted"@en ;
    skos:definition "Capability for recognising emotions based on biometrics information"@en ;
    skos:prefLabel "Biometric Emotion Recognition"@en .

ai-owl:BiometricIdentification a rdfs:Class,
        owl:Class,
        ai-owl:Capability ;
    dct:contributor _:person-delaram-golpayegani ;
    dct:created "2024-12-01"^^xsd:date ;
    dct:source [ a schema:WebPage ;
            schema:name "The AI Act Recital 15" ;
            schema:url "https://eur-lex.europa.eu/legal-content/EN/TXT/HTML/?uri=OJ:L_202401689#rct_15" ] ;
    rdfs:isDefinedBy ai-owl: ;
    rdfs:subClassOf ai-owl:BiometricCapability,
        ai-owl:HumanIdentification ;
    sw:term_status "accepted"@en ;
    skos:definition "Capability involving automated recognition of physical, physiological and behavioural human features such as the face, eye movement, body shape, voice, prosody, gait, posture, heart rate, blood pressure, odour, keystrokes characteristics, for the purpose of establishing an individual’s identity by comparing biometric data of that individual to stored biometric data of individuals in a reference database, irrespective of whether the individual has given its consent or not"@en ;
    skos:prefLabel "Biometric Identification"@en .

ai-owl:ChatbotCapability a rdfs:Class,
        owl:Class,
        ai-owl:Capability ;
    dct:contributor _:person-delaram-golpayegani,
        _:person-harshvardhan-j-pandit ;
    dct:created "2025-12-17"^^xsd:date ;
    dct:source _:b91869a137134d7183222578424a7bdbb ;
    rdfs:isDefinedBy ai-owl: ;
    rdfs:subClassOf ai-owl:NaturalLanguageProcessing ;
    sw:term_status "accepted"@en ;
    skos:definition "Capability to simulate human-like conversation with a user through messaging platforms, websites, mobile apps, or telephone systems, often employing natural language processing and machine learning to engage in conversation mimicking human interaction"@en ;
    skos:prefLabel "Chatbot Capability"@en .

ai-owl:ComputationalCreativity a rdfs:Class,
        owl:Class,
        ai-owl:Capability ;
    dct:contributor _:person-delaram-golpayegani,
        _:person-harshvardhan-j-pandit ;
    dct:created "2025-12-17"^^xsd:date ;
    dct:source _:b91869a137134d7183222578424a7bdbb ;
    rdfs:isDefinedBy ai-owl: ;
    rdfs:subClassOf ai-owl:HumanOrientedCapability ;
    sw:term_status "accepted"@en ;
    skos:definition "computer systems that emulate human creative processes and produce artistic, design output that simulates innovation and originality"@en ;
    skos:prefLabel "Computational Creativity"@en .

ai-owl:ComputerVision a rdfs:Class,
        owl:Class,
        ai-owl:Capability ;
    dct:contributor _:person-delaram-golpayegani ;
    dct:created "2024-12-01"^^xsd:date ;
    dct:source "ISO/IEC 22989:2022 3.7.1"@en ;
    rdfs:isDefinedBy ai-owl: ;
    rdfs:subClassOf ai-owl:Capability ;
    sw:term_status "accepted"@en ;
    skos:definition "Capability of a functional unit to acquire, process and interpret data representing images or video"@en ;
    skos:prefLabel "Computer Vision"@en .

ai-owl:ContentBasedRetrieval a rdfs:Class,
        owl:Class,
        ai-owl:Capability ;
    dct:contributor _:person-harshvardhan-j-pandit ;
    dct:created "2024-12-01"^^xsd:date ;
    rdfs:isDefinedBy ai-owl: ;
    rdfs:subClassOf ai-owl:InformationRetrieval ;
    sw:term_status "accepted"@en ;
    skos:definition "Capability for retrieval of information using the actual content to identify, select, filter, and provide results"@en ;
    skos:prefLabel "Content-based Retrieval"@en .

ai-owl:ContentGeneration a rdfs:Class,
        owl:Class,
        ai-owl:Capability ;
    dct:contributor _:person-delaram-golpayegani,
        _:person-harshvardhan-j-pandit ;
    dct:created "2024-12-01"^^xsd:date ;
    rdfs:isDefinedBy ai-owl: ;
    rdfs:subClassOf ai-owl:Capability ;
    sw:term_status "accepted"@en ;
    skos:definition "Capability to generate new content that is distinct from merely deriving or transforming existing content"@en ;
    skos:prefLabel "Content Generation"@en .

ai-owl:ContextAwareRetrieval a rdfs:Class,
        owl:Class,
        ai-owl:Capability ;
    dct:contributor _:person-harshvardhan-j-pandit ;
    dct:created "2024-12-01"^^xsd:date ;
    rdfs:isDefinedBy ai-owl: ;
    rdfs:subClassOf ai-owl:InformationRetrieval ;
    sw:term_status "accepted"@en ;
    skos:definition "Capability for retrieval of information that takes into account the user's context such as e.g., location, time, device, or activity to provide more relevant results"@en ;
    skos:prefLabel "Context-aware Retrieval"@en .

ai-owl:DialogueManagement a rdfs:Class,
        owl:Class,
        ai-owl:Capability ;
    dct:contributor _:person-delaram-golpayegani ;
    dct:created "2024-12-01"^^xsd:date ;
    dct:source "ISO/IEC 22989:2022 3.6.14"@en ;
    rdfs:isDefinedBy ai-owl: ;
    rdfs:subClassOf ai-owl:LanguageCapability ;
    sw:term_status "accepted"@en ;
    skos:definition "Capability for shortening a portion of content such as text while retaining important semantic information"@en ;
    skos:prefLabel "Dialogue Management"@en .

ai-owl:EmotionRecognition a rdfs:Class,
        owl:Class,
        ai-owl:Capability ;
    dct:contributor _:person-delaram-golpayegani ;
    dct:created "2024-12-01"^^xsd:date ;
    dct:source "ISO/IEC 22989:2022 3.6.3"@en ;
    rdfs:isDefinedBy ai-owl: ;
    rdfs:subClassOf ai-owl:HumanOrientedCapability ;
    sw:term_status "accepted"@en ;
    skos:definition "Capability for identifying and categorising emotions expressed in a piece of text, speech, video or image or combination thereof"@en ;
    skos:prefLabel "Emotion Recognition"@en .

ai-owl:FaceRecognition a rdfs:Class,
        owl:Class,
        ai-owl:Capability ;
    dct:contributor _:person-delaram-golpayegani ;
    dct:created "2024-12-01"^^xsd:date ;
    dct:source "ISO/IEC 22989:2022 3.7.2"@en ;
    rdfs:isDefinedBy ai-owl: ;
    rdfs:subClassOf ai-owl:BiometricCapability,
        ai-owl:ComputerVision ;
    sw:term_status "accepted"@en ;
    skos:definition "Capability involving automatic pattern recognition for comparing stored images of human faces with the image of an actual face, indicating any matching, if it exists, and any data, if they exist, identifying the person to whom the face belongs"@en ;
    skos:prefLabel "Face Recognition"@en ;
    skos:scopeNote "EU Vocabularies' AI taxonomy defines 'Facial Recognition as \"computer vision technology employing biometric analysis and mapping of facial characteristics for facial identification purposes, recognising and verifying an individual's identity\", which not only refers to the capability for face recognition but also indicates the *purposes* for which this is being used. In DPV, such purposes are defined separately within the main DPV"@en .

ai-owl:GestureRecognition a rdfs:Class,
        owl:Class,
        ai-owl:Capability ;
    dct:contributor _:person-delaram-golpayegani ;
    dct:created "2024-12-01"^^xsd:date ;
    dct:source " Defining Artificial Intelligence 2.0"@en,
        "AI Watch"@en ;
    rdfs:isDefinedBy ai-owl: ;
    rdfs:subClassOf ai-owl:BiometricCapability,
        ai-owl:ComputerVision ;
    sw:term_status "accepted"@en ;
    skos:definition "Capability for recognising human gestures"@en ;
    skos:prefLabel "Gesture Recognition"@en .

ai-owl:HumanIdentification a rdfs:Class,
        owl:Class,
        ai-owl:Capability ;
    dct:contributor _:person-delaram-golpayegani,
        _:person-harshvardhan-j-pandit ;
    dct:created "2026-02-09"^^xsd:date ;
    rdfs:isDefinedBy ai-owl: ;
    rdfs:subClassOf ai-owl:HumanOrientedCapability ;
    sw:term_status "accepted"@en ;
    skos:definition "Capability of a system that identifies a human whether at an individual or group level"@en ;
    skos:prefLabel "Human Identification"@en .

ai-owl:HumanOrientedCapability a rdfs:Class,
        owl:Class,
        ai-owl:Capability ;
    dct:contributor _:person-harshvardhan-j-pandit ;
    dct:created "2024-12-01"^^xsd:date ;
    rdfs:isDefinedBy ai-owl: ;
    rdfs:subClassOf ai-owl:Capability ;
    sw:term_status "accepted"@en ;
    skos:definition "Capabilities that are inherently about humans or oriented towards human characteristics and activities"@en ;
    skos:prefLabel "Human-Oriented Capability"@en .

ai-owl:ImageClassification a rdfs:Class,
        owl:Class,
        ai-owl:Capability ;
    dct:contributor _:person-delaram-golpayegani,
        _:person-harshvardhan-j-pandit ;
    dct:created "2025-12-17"^^xsd:date ;
    dct:source _:b91869a137134d7183222578424a7bdbb ;
    rdfs:isDefinedBy ai-owl: ;
    rdfs:subClassOf ai-owl:ComputerVision ;
    sw:term_status "accepted"@en ;
    skos:definition "Capability of categorising and labelling groups of pixels or vectors within an image based on particular rules, involving the assignment of images to predefined classes or categories"@en ;
    skos:prefLabel "Image Classification"@en .

ai-owl:ImageGeneration a rdfs:Class,
        owl:Class,
        ai-owl:Capability ;
    dct:contributor _:person-delaram-golpayegani,
        _:person-harshvardhan-j-pandit ;
    dct:created "2024-12-01"^^xsd:date ;
    rdfs:isDefinedBy ai-owl: ;
    rdfs:subClassOf ai-owl:ContentGeneration ;
    sw:term_status "accepted"@en ;
    skos:definition "Capability to generate image"@en ;
    skos:prefLabel "Image Generation"@en .

ai-owl:ImageRecognition a rdfs:Class,
        owl:Class,
        ai-owl:Capability ;
    dct:contributor _:person-delaram-golpayegani ;
    dct:created "2024-12-01"^^xsd:date ;
    dct:source "ISO/IEC 22989:2022 3.7.4"@en ;
    rdfs:isDefinedBy ai-owl: ;
    rdfs:subClassOf ai-owl:ComputerVision ;
    sw:term_status "accepted"@en ;
    skos:definition "Capability for image classification process that classifies object(s), pattern(s) or concept(s) in an image"@en ;
    skos:prefLabel "Image Recognition"@en .

ai-owl:InformationRetrieval a rdfs:Class,
        owl:Class,
        ai-owl:Capability ;
    dct:contributor _:person-delaram-golpayegani ;
    dct:created "2024-12-01"^^xsd:date ;
    dct:source "ISO/IEC 22989:2022 3.6.4"@en ;
    rdfs:isDefinedBy ai-owl: ;
    rdfs:subClassOf ai-owl:Capability ;
    sw:term_status "accepted"@en ;
    skos:definition "Capability for retrieving relevant documents or parts of documents from a dataset, typically based on keyword or natural language queries"@en ;
    skos:prefLabel "Information Retrieval (IR)"@en .

ai-owl:LanguageCapability a rdfs:Class,
        owl:Class,
        ai-owl:Capability ;
    dct:contributor _:person-harshvardhan-j-pandit ;
    dct:created "2024-12-01"^^xsd:date ;
    rdfs:isDefinedBy ai-owl: ;
    rdfs:subClassOf ai-owl:Capability ;
    sw:term_status "accepted"@en ;
    skos:definition "Capabilities related to languages"@en ;
    skos:prefLabel "Language Capability"@en .

ai-owl:LieDetection a rdfs:Class,
        owl:Class,
        ai-owl:Capability ;
    dct:contributor _:person-delaram-golpayegani ;
    dct:created "2024-12-01"^^xsd:date ;
    rdfs:isDefinedBy ai-owl: ;
    rdfs:subClassOf ai-owl:HumanOrientedCapability ;
    sw:term_status "accepted"@en ;
    skos:definition "Capability to detect lies in the context of human speech, behaviour, information, or activities"@en ;
    skos:prefLabel "Lie Detection"@en .

ai-owl:LocalBiometricIdentification a rdfs:Class,
        owl:Class,
        ai-owl:Capability ;
    dct:contributor _:person-harshvardhan-j-pandit ;
    dct:created "2024-12-01"^^xsd:date ;
    rdfs:isDefinedBy ai-owl: ;
    rdfs:subClassOf ai-owl:BiometricIdentification ;
    sw:term_status "accepted"@en ;
    skos:definition "Capability involving biometric identification carried out locally"@en ;
    skos:prefLabel "Local Biometric Identification"@en .

ai-owl:MachineTranslation a rdfs:Class,
        owl:Class,
        ai-owl:Capability ;
    dct:contributor _:person-delaram-golpayegani ;
    dct:created "2024-12-01"^^xsd:date ;
    dct:source "ISO/IEC 22989:2022 3.6.5"@en ;
    rdfs:isDefinedBy ai-owl: ;
    rdfs:subClassOf ai-owl:LanguageCapability ;
    sw:term_status "accepted"@en ;
    skos:definition "Capability for automated translation of text or speech from one natural language to another using a computer system"@en ;
    skos:prefLabel "Machine Translation"@en .

ai-owl:MotionAnalysis a rdfs:Class,
        owl:Class,
        ai-owl:Capability ;
    dct:contributor _:person-delaram-golpayegani,
        _:person-harshvardhan-j-pandit ;
    dct:created "2025-12-17"^^xsd:date ;
    dct:source _:b91869a137134d7183222578424a7bdbb ;
    rdfs:isDefinedBy ai-owl: ;
    rdfs:subClassOf ai-owl:ComputerVision ;
    sw:term_status "accepted"@en ;
    skos:definition "Capability of deriving meaningful information about motion from visual data, including tracking objects across frames, analysing trajectories, estimating velocity and acceleration, and interpreting the meaning of motion patterns"@en ;
    skos:prefLabel "Motion Analysis"@en .

ai-owl:MultiModalRetrieval a rdfs:Class,
        owl:Class,
        ai-owl:Capability ;
    dct:contributor _:person-harshvardhan-j-pandit ;
    dct:created "2024-12-01"^^xsd:date ;
    rdfs:isDefinedBy ai-owl: ;
    rdfs:subClassOf ai-owl:InformationRetrieval ;
    sw:term_status "accepted"@en ;
    skos:definition "Capability for retrieval of information using multiple modalities such as text, images, audio, and video and supporting cross-modal queries such as taking text as input to search images"@en ;
    skos:prefLabel "Multi-modal Retrieval"@en .

ai-owl:MusicInformationRetrieval a rdfs:Class,
        owl:Class,
        ai-owl:Capability ;
    dct:contributor _:person-delaram-golpayegani ;
    dct:created "2024-12-01"^^xsd:date ;
    dct:source " Defining Artificial Intelligence 2.0"@en,
        "AI Watch"@en ;
    rdfs:isDefinedBy ai-owl: ;
    rdfs:subClassOf ai-owl:InformationRetrieval ;
    sw:term_status "accepted"@en ;
    skos:definition "Capability for retrieving, analysing, and categorising music-related information such as audio files, melodies, or lyrics using audio features, metadata, and user queries"@en ;
    skos:prefLabel "Music Information Retrieval (MIR)"@en .

ai-owl:NamedEntityRecognition a rdfs:Class,
        owl:Class,
        ai-owl:Capability ;
    dct:contributor _:person-delaram-golpayegani ;
    dct:created "2024-12-01"^^xsd:date ;
    dct:source "ISO/IEC 22989:2022 3.6.6"@en ;
    rdfs:isDefinedBy ai-owl: ;
    rdfs:subClassOf ai-owl:LanguageCapability ;
    sw:term_status "accepted"@en ;
    skos:definition "Capability for recognising and labelling the denotational names of entities and their categories for sequences of words in a stream of text or speech"@en ;
    skos:prefLabel "Named Entity Recognition"@en .

ai-owl:NaturalLanguageGeneration a rdfs:Class,
        owl:Class,
        ai-owl:Capability ;
    dct:contributor _:person-delaram-golpayegani ;
    dct:created "2024-12-01"^^xsd:date ;
    dct:source "ISO/IEC 22989:2022 3.6.8"@en ;
    rdfs:isDefinedBy ai-owl: ;
    rdfs:subClassOf ai-owl:LanguageCapability ;
    sw:term_status "accepted"@en ;
    skos:definition "Converting data carrying semantics into natural language"@en ;
    skos:prefLabel "Natural Language Generation"@en .

ai-owl:NaturalLanguageProcessing a rdfs:Class,
        owl:Class,
        ai-owl:Capability ;
    dct:contributor _:person-delaram-golpayegani,
        _:person-harshvardhan-j-pandit ;
    dct:created "2025-12-17"^^xsd:date ;
    dct:source _:b91869a137134d7183222578424a7bdbb ;
    rdfs:isDefinedBy ai-owl: ;
    rdfs:subClassOf ai-owl:LanguageCapability ;
    sw:term_status "accepted"@en ;
    skos:definition "Capability enabling computers to understand and communicate with human language"@en ;
    skos:prefLabel "Natural Language Processing"@en .

ai-owl:ObjectDetection a rdfs:Class,
        owl:Class,
        ai-owl:Capability ;
    dct:contributor _:person-delaram-golpayegani,
        _:person-harshvardhan-j-pandit ;
    dct:created "2025-12-17"^^xsd:date ;
    dct:source _:b91869a137134d7183222578424a7bdbb ;
    rdfs:isDefinedBy ai-owl: ;
    rdfs:subClassOf ai-owl:ComputerVision ;
    sw:term_status "accepted"@en ;
    skos:definition "computer vision technology that detects instances of semantic objects in digital images and videos, covering domains like face detection and pedestrian detection, with applications spanning image retrieval and video surveillance"@en ;
    skos:prefLabel "Object Detection"@en .

ai-owl:ObjectRecognition a rdfs:Class,
        owl:Class,
        ai-owl:Capability ;
    dct:contributor _:person-delaram-golpayegani ;
    dct:created "2024-12-01"^^xsd:date ;
    dct:source " Defining Artificial Intelligence 2.0"@en,
        "AI Watch"@en ;
    rdfs:isDefinedBy ai-owl: ;
    rdfs:subClassOf ai-owl:ComputerVision ;
    sw:term_status "accepted"@en ;
    skos:definition "Capability to recognise objects"@en ;
    skos:prefLabel "Object Recognition"@en .

ai-owl:PartOfSpeechTagging a rdfs:Class,
        owl:Class,
        ai-owl:Capability ;
    dct:contributor _:person-delaram-golpayegani ;
    dct:created "2024-12-01"^^xsd:date ;
    dct:source "ISO/IEC 22989:2022 3.6.13"@en ;
    rdfs:isDefinedBy ai-owl: ;
    rdfs:subClassOf ai-owl:LanguageCapability ;
    sw:term_status "accepted"@en ;
    skos:definition "Capability for assigning a category (e.g. verb, noun, adjective) to a word based on its grammatical properties"@en ;
    skos:prefLabel "Part Of Speech Tagging"@en .

ai-owl:PatternRecognition a rdfs:Class,
        owl:Class,
        ai-owl:Capability ;
    dct:contributor _:person-delaram-golpayegani,
        _:person-harshvardhan-j-pandit ;
    dct:created "2025-12-17"^^xsd:date ;
    dct:source _:b91869a137134d7183222578424a7bdbb ;
    rdfs:isDefinedBy ai-owl: ;
    rdfs:subClassOf ai-owl:ComputerVision ;
    sw:term_status "accepted"@en ;
    skos:definition "Capability for automated identification of patterns and regularities in data, utilising algorithms to detect patterns or regularities for categorising data into distinct groups, encompassing diverse applications such as image analysis, speech processing, and biometric authentication"@en ;
    skos:prefLabel "Pattern Recognition"@en .

ai-owl:PerceptionBasedAI a rdfs:Class,
        owl:Class,
        ai-owl:Capability ;
    dct:contributor _:person-delaram-golpayegani,
        _:person-harshvardhan-j-pandit ;
    dct:created "2025-12-17"^^xsd:date ;
    dct:source _:b91869a137134d7183222578424a7bdbb ;
    rdfs:isDefinedBy ai-owl: ;
    rdfs:subClassOf ai-owl:ComputerVision ;
    sw:term_status "accepted"@en ;
    skos:definition "Capability of using agents to interpret and understand information from their environment through sensory inputs"@en ;
    skos:prefLabel "Perception-based AI"@en .

ai-owl:PersonalityTraitAnalysis a rdfs:Class,
        owl:Class,
        ai-owl:Capability ;
    dct:contributor _:person-delaram-golpayegani ;
    dct:created "2024-12-01"^^xsd:date ;
    rdfs:isDefinedBy ai-owl: ;
    rdfs:subClassOf ai-owl:HumanOrientedCapability ;
    sw:term_status "accepted"@en ;
    skos:definition "Capability for determining and analysing people's personality traits"@en ;
    skos:prefLabel "Personality Trait Analysis"@en .

ai-owl:PostTimeBiometricIdentification a rdfs:Class,
        owl:Class,
        ai-owl:Capability ;
    dct:contributor _:person-harshvardhan-j-pandit ;
    dct:created "2024-12-01"^^xsd:date ;
    rdfs:isDefinedBy ai-owl: ;
    rdfs:subClassOf ai-owl:BiometricIdentification ;
    sw:term_status "accepted"@en ;
    skos:definition "Capability involving biometric identification carried out later or not in real-time or non-instantaneously"@en ;
    skos:prefLabel "Post-Time Biometric Identification"@en .

ai-owl:Profiling a rdfs:Class,
        owl:Class,
        ai-owl:Capability ;
    dct:contributor _:person-delaram-golpayegani ;
    dct:created "2024-12-01"^^xsd:date ;
    rdfs:isDefinedBy ai-owl: ;
    rdfs:subClassOf ai-owl:HumanOrientedCapability,
        dpv-owl:Profiling ;
    sw:term_status "accepted"@en ;
    skos:definition "Capability where AI is used to construct a profile of an individual (human) or a group of individuals"@en ;
    skos:prefLabel "Profiling"@en .

ai-owl:QuestionAnswering a rdfs:Class,
        owl:Class,
        ai-owl:Capability ;
    dct:contributor _:person-delaram-golpayegani ;
    dct:created "2024-12-01"^^xsd:date ;
    dct:source "ISO/IEC 22989:2022 3.6.14"@en ;
    rdfs:isDefinedBy ai-owl: ;
    rdfs:subClassOf ai-owl:LanguageCapability ;
    sw:term_status "accepted"@en ;
    skos:definition "Capability for determining the most appropriate answer to a question provided in natural language"@en ;
    skos:prefLabel "Question Answering"@en .

ai-owl:RealTimeBiometricIdentification a rdfs:Class,
        owl:Class,
        ai-owl:Capability ;
    dct:contributor _:person-delaram-golpayegani ;
    dct:created "2024-12-01"^^xsd:date ;
    rdfs:isDefinedBy ai-owl: ;
    rdfs:subClassOf ai-owl:BiometricIdentification ;
    sw:term_status "accepted"@en ;
    skos:definition "Capability involving biometric identification carried out in real-time or instantaneously"@en ;
    skos:prefLabel "Real-Time Biometric Identification"@en .

ai-owl:RelationshipExtraction a rdfs:Class,
        owl:Class,
        ai-owl:Capability ;
    dct:contributor _:person-delaram-golpayegani ;
    dct:created "2024-12-01"^^xsd:date ;
    dct:source "ISO/IEC 22989:2022 3.6.15"@en ;
    rdfs:isDefinedBy ai-owl: ;
    rdfs:subClassOf ai-owl:LanguageCapability ;
    sw:term_status "accepted"@en ;
    skos:definition "Capability for identifying relationships among entities mentioned in a text"@en ;
    skos:prefLabel "Relationship Extraction"@en .

ai-owl:RemoteBiometricIdentification a rdfs:Class,
        owl:Class,
        ai-owl:Capability ;
    dct:contributor _:person-delaram-golpayegani ;
    dct:created "2024-12-01"^^xsd:date ;
    rdfs:isDefinedBy ai-owl: ;
    rdfs:subClassOf ai-owl:BiometricIdentification ;
    sw:term_status "accepted"@en ;
    skos:definition "Capability involving biometric identification carried out remotely"@en ;
    skos:prefLabel "Remote Biometric Identification"@en .

ai-owl:RemoteSensing a rdfs:Class,
        owl:Class,
        ai-owl:Capability ;
    dct:contributor _:person-delaram-golpayegani,
        _:person-harshvardhan-j-pandit ;
    dct:created "2025-12-17"^^xsd:date ;
    dct:source _:b91869a137134d7183222578424a7bdbb ;
    rdfs:isDefinedBy ai-owl: ;
    rdfs:subClassOf ai-owl:PerceptionBasedAI ;
    sw:term_status "accepted"@en ;
    skos:definition "Capability for acquisition of information about an object or phenomenon without physical contact, typically using aerial sensor technologies"@en ;
    skos:prefLabel "Remote Sensing"@en .

ai-owl:SentimentAnalysis a rdfs:Class,
        owl:Class,
        ai-owl:Capability ;
    dct:contributor _:person-delaram-golpayegani ;
    dct:created "2024-12-01"^^xsd:date ;
    dct:source "ISO/IEC 22989:2022 3.6.16"@en ;
    rdfs:isDefinedBy ai-owl: ;
    rdfs:subClassOf ai-owl:HumanOrientedCapability,
        ai-owl:LanguageCapability ;
    sw:term_status "accepted"@en ;
    skos:definition "Capability for computationally identifying and categorising opinions expressed in a piece of text, speech or image, to determine a range of feeling such as from positive to negative"@en ;
    skos:prefLabel "Sentiment Analysis"@en .

ai-owl:SoundSourceSeparation a rdfs:Class,
        owl:Class,
        ai-owl:Capability ;
    dct:contributor _:person-delaram-golpayegani ;
    dct:created "2024-12-01"^^xsd:date ;
    dct:source " Defining Artificial Intelligence 2.0"@en,
        "AI Watch"@en ;
    rdfs:isDefinedBy ai-owl: ;
    rdfs:subClassOf ai-owl:AudioCapability ;
    sw:term_status "accepted"@en ;
    skos:definition "Capability for extracting individual sound from audio recordings"@en ;
    skos:prefLabel "Sound Source Separation"@en .

ai-owl:SoundSynthesis a rdfs:Class,
        owl:Class,
        ai-owl:Capability ;
    dct:contributor _:person-delaram-golpayegani ;
    dct:created "2024-12-01"^^xsd:date ;
    dct:source " Defining Artificial Intelligence 2.0"@en,
        "AI Watch"@en ;
    rdfs:isDefinedBy ai-owl: ;
    rdfs:subClassOf ai-owl:AudioCapability,
        ai-owl:ContentGeneration ;
    sw:term_status "accepted"@en ;
    skos:definition "Capability for generation of artificial sound"@en ;
    skos:prefLabel "Sound Synthesis"@en .

ai-owl:SpeakerRecognition a rdfs:Class,
        owl:Class,
        ai-owl:Capability ;
    dct:contributor _:person-delaram-golpayegani ;
    dct:created "2024-12-01"^^xsd:date ;
    dct:source " Defining Artificial Intelligence 2.0"@en,
        "AI Watch"@en ;
    rdfs:isDefinedBy ai-owl: ;
    rdfs:subClassOf ai-owl:AudioProcessing,
        ai-owl:HumanOrientedCapability ;
    sw:term_status "accepted"@en ;
    skos:definition "Capability of recognising speaker(s) in audio recordings"@en ;
    skos:prefLabel "Speaker Recognition"@en .

ai-owl:SpeechRecognition a rdfs:Class,
        owl:Class,
        ai-owl:Capability ;
    dct:contributor _:person-delaram-golpayegani ;
    dct:created "2024-12-01"^^xsd:date ;
    dct:source "ISO/IEC 22989:2022 3.6.17"@en ;
    rdfs:isDefinedBy ai-owl: ;
    rdfs:subClassOf ai-owl:AudioProcessing,
        ai-owl:HumanOrientedCapability ;
    sw:term_status "accepted"@en ;
    skos:definition "Capability of converting a speech signal to a representation of the content of the speech"@en ;
    skos:prefLabel "Speech Recognition"@en .

ai-owl:SpeechSynthesis a rdfs:Class,
        owl:Class,
        ai-owl:Capability ;
    dct:contributor _:person-delaram-golpayegani ;
    dct:created "2024-12-01"^^xsd:date ;
    dct:source "ISO/IEC 22989:2022 3.6.18"@en ;
    rdfs:isDefinedBy ai-owl: ;
    rdfs:subClassOf ai-owl:AudioCapability,
        ai-owl:ContentGeneration ;
    sw:term_status "accepted"@en ;
    skos:definition "Capability for generation of artificial speech"@en ;
    skos:prefLabel "Speech Synthesis"@en .

ai-owl:TextClassification a rdfs:Class,
        owl:Class,
        ai-owl:Capability ;
    dct:contributor _:person-delaram-golpayegani,
        _:person-harshvardhan-j-pandit ;
    dct:created "2025-12-17"^^xsd:date ;
    dct:source _:b91869a137134d7183222578424a7bdbb ;
    rdfs:isDefinedBy ai-owl: ;
    rdfs:subClassOf ai-owl:NaturalLanguageProcessing ;
    sw:term_status "accepted"@en ;
    skos:definition "Capability of assigning predefined labels to text data in order to automatically categorise it into groups"@en ;
    skos:prefLabel "Text Classification"@en .

ai-owl:TextDataMining a rdfs:Class,
        owl:Class,
        ai-owl:Capability ;
    dct:contributor _:person-delaram-golpayegani,
        _:person-harshvardhan-j-pandit ;
    dct:created "2025-12-17"^^xsd:date ;
    dct:source _:b91869a137134d7183222578424a7bdbb ;
    rdfs:isDefinedBy ai-owl: ;
    rdfs:subClassOf ai-owl:NaturalLanguageProcessing ;
    sw:term_status "accepted"@en ;
    skos:definition "Capability of selecting and analysing large amounts of text or data resources to discover patterns, relationships, and semantic insights that provide valuable information for research and decision-making"@en ;
    skos:prefLabel "Text and Data Mining"@en .

ai-owl:VideoGeneration a rdfs:Class,
        owl:Class,
        ai-owl:Capability ;
    dct:contributor _:person-delaram-golpayegani,
        _:person-harshvardhan-j-pandit ;
    dct:created "2024-12-01"^^xsd:date ;
    rdfs:isDefinedBy ai-owl: ;
    rdfs:subClassOf ai-owl:ContentGeneration ;
    sw:term_status "accepted"@en ;
    skos:definition "Capability to generate video"@en ;
    skos:prefLabel "Video Generation"@en .

ai-owl:VisualRecognition a rdfs:Class,
        owl:Class,
        ai-owl:Capability ;
    dct:contributor _:person-delaram-golpayegani,
        _:person-harshvardhan-j-pandit ;
    dct:created "2025-12-17"^^xsd:date ;
    dct:source _:b91869a137134d7183222578424a7bdbb ;
    rdfs:isDefinedBy ai-owl: ;
    rdfs:subClassOf ai-owl:ComputerVision ;
    sw:term_status "accepted"@en ;
    skos:definition "Capability that identifies and categorises objects, scenes, activities, and other visual elements in images or video, and includes image classification, object detection, scene understanding, and visual pattern recognition"@en ;
    skos:prefLabel "Visual Recognition"@en .

ai-owl:serialisation-html a profile:ResourceDescriptor ;
    dct:conformsTo <https://www.w3.org/TR/html/> ;
    dct:format <https://www.iana.org/assignments/media-types/text/html> ;
    dct:title "AI Technology Concepts - HTML serialisation" ;
    profile:hasArtifact <https://w3id.org/dpv/ai/ai-owl.html> ;
    profile:hasRole role:specification .

ai-owl:serialisation-jsonld a profile:ResourceDescriptor ;
    dct:conformsTo <https://www.w3.org/TR/json-ld11/> ;
    dct:format <https://www.iana.org/assignments/media-types/application/ld+json> ;
    dct:title "AI Technology Concepts - JSON-LD serialisation" ;
    profile:hasArtifact <https://w3id.org/dpv/ai/ai-owl.jsonld> ;
    profile:hasRole role:vocabulary .

ai-owl:serialisation-n3 a profile:ResourceDescriptor ;
    dct:conformsTo <https://www.w3.org/TeamSubmission/n3/> ;
    dct:format <https://www.iana.org/assignments/media-types/text/n3> ;
    dct:title "AI Technology Concepts - N3 serialisation" ;
    profile:hasArtifact <https://w3id.org/dpv/ai/ai-owl.n3> ;
    profile:hasRole role:vocabulary .

ai-owl:serialisation-rdf a profile:ResourceDescriptor ;
    dct:conformsTo rdf: ;
    dct:format <https://www.iana.org/assignments/media-types/application/rdf+xml> ;
    dct:title "AI Technology Concepts - RDF/XML serialisation" ;
    profile:hasArtifact <https://w3id.org/dpv/ai/ai-owl.rdf> ;
    profile:hasRole role:vocabulary .

ai-owl:serialisation-ttl a profile:ResourceDescriptor ;
    dct:conformsTo <https://www.w3.org/TR/turtle/> ;
    dct:format <https://www.iana.org/assignments/media-types/text/turtle> ;
    dct:title "AI Technology Concepts - Turtle serialisation" ;
    profile:hasArtifact <https://w3id.org/dpv/ai/ai-owl.ttl> ;
    profile:hasRole role:vocabulary .

<https://w3id.org/dpv/examples> a profile:ResourceDescriptor ;
    dct:conformsTo <https://www.w3.org/TR/html/> ;
    dct:format <https://www.iana.org/assignments/media-types/text/html> ;
    dct:title "Examples" ;
    profile:hasArtifact <https://w3id.org/dpv/examples> ;
    profile:hasRole role:guidance .

<https://w3id.org/dpv/guides> a profile:ResourceDescriptor ;
    dct:conformsTo <https://www.w3.org/TR/html/> ;
    dct:format <https://www.iana.org/assignments/media-types/text/html> ;
    dct:title "Guides for Data Privacy Vocabulary" ;
    profile:hasArtifact <https://w3id.org/dpv/guides> ;
    profile:hasRole role:guidance .

<https://w3id.org/dpv/primer> a profile:ResourceDescriptor ;
    dct:conformsTo <https://www.w3.org/TR/html/> ;
    dct:format <https://www.iana.org/assignments/media-types/text/html> ;
    dct:title "Primer for Data Privacy Vocabulary" ;
    profile:hasArtifact <https://w3id.org/dpv/primer> ;
    profile:hasRole role:guidance .

ai-owl: a owl:Ontology,
        profile:Profile ;
    dct:bibliographicCitation "Harshvardhan J. Pandit, Beatriz Esteves, Georg P. Krog, Paul Ryan, Delaram Golpayegani, Julian Flake (2025) Data Privacy Vocabulary (DPV) – Version 2.0. In: Demartini, G., et al. The Semantic Web – ISWC 2024. ISWC 2024. Lecture Notes in Computer Science, vol 15233. Springer, Cham. https://doi.org/10.1007/978-3-031-77847-6_10" ;
    dct:conformsTo <http://www.w3.org/2002/07/owl>,
        "http://www.w3.org/2000/01/rdf-schema",
        "http://www.w3.org/2004/02/skos/core" ;
    dct:contributor _:person-delaram-golpayegani,
        _:person-harshvardhan-j-pandit ;
    dct:created "2024-05-31"@en ;
    dct:creator _:person-delaram-golpayegani,
        _:person-harshvardhan-j-pandit ;
    dct:description "Extension to the Data Privacy Vocabulary (DPV) providing concepts for representing information about AI technologies"@en ;
    dct:hasVersion ai-owl: ;
    dct:identifier "https://w3id.org/dpv/ai" ;
    dct:issued "2024-05-31"@en ;
    dct:license <https://www.w3.org/copyright/document-license-2023/> ;
    dct:modified "2026-02-25"@en ;
    dct:publisher <https://www.w3.org/> ;
    dct:source <https://www.w3.org/groups/cg/dpvcg/> ;
    dct:title "AI Technology Concepts"@en ;
    bibo:doi "10.5281/zenodo.12505841" ;
    bibo:status "http://purl.org/ontology/bibo/status/published" ;
    vann:preferredNamespacePrefix "ai" ;
    vann:preferredNamespaceUri "https://w3id.org/dpv/ai#" ;
    rdfs:Label "AI"@en ;
    owl:versionIRI <https://w3id.org/dpv/2.3/ai/owl#> ;
    owl:versionInfo "2.3" ;
    profile:hasResource ai-owl:serialisation-html,
        ai-owl:serialisation-jsonld,
        ai-owl:serialisation-n3,
        ai-owl:serialisation-rdf,
        ai-owl:serialisation-ttl,
        <https://w3id.org/dpv/examples>,
        <https://w3id.org/dpv/guides>,
        <https://w3id.org/dpv/primer> ;
    profile:isProfileOf <http://www.w3.org/2002/07/owl>,
        ai-owl:,
        <https://w3id.org/dpv/tech/owl> ;
    foaf:logo <https://w3id.org/dpv/media/logo.png> ;
    schema:version "2.3" .

_:org-adapt-centre-trinity-college-dublin a foaf:Organization ;
    foaf:name "ADAPT Centre, Trinity College Dublin" .

_:org-ai-accountability-lab-aial-trinity-college-dublin a foaf:Organization ;
    foaf:name "AI Accountability Lab (AIAL), Trinity College Dublin" .

_:b91869a137134d7183222578424a7bdbb a schema:WebPage ;
    schema:name "AI Taxonomy - EU Vocabularies" ;
    schema:url "http://data.europa.eu/8s8/ai-taxonomy" .

_:person-harshvardhan-j-pandit a dct:Agent,
        foaf:Person ;
    scoro:hasORCID "0000-0002-5068-3714" ;
    org:memberOf _:org-ai-accountability-lab-aial-trinity-college-dublin ;
    foaf:homepage "https://harshp.com/" ;
    foaf:name "Harshvardhan J. Pandit" .

_:person-delaram-golpayegani a dct:Agent,
        foaf:Person ;
    scoro:hasORCID "0000-0002-1208-186X" ;
    org:memberOf _:org-adapt-centre-trinity-college-dublin ;
    foaf:name "Delaram Golpayegani" .

