@prefix bibo: <http://purl.org/ontology/bibo/> .
@prefix dct: <http://purl.org/dc/terms/> .
@prefix dpv-owl: <https://w3id.org/dpv/owl#> .
@prefix foaf: <http://xmlns.com/foaf/0.1/> .
@prefix org: <http://www.w3.org/ns/org#> .
@prefix owl: <http://www.w3.org/2002/07/owl#> .
@prefix profile: <http://www.w3.org/ns/dx/prof/> .
@prefix rdf: <http://www.w3.org/1999/02/22-rdf-syntax-ns#> .
@prefix rdfs: <http://www.w3.org/2000/01/rdf-schema#> .
@prefix role: <http://www.w3.org/ns/dx/prof/role/> .
@prefix schema: <https://schema.org/> .
@prefix scoro: <http://purl.org/spar/scoro/> .
@prefix sector-health-owl: <https://w3id.org/dpv/sector/health/owl#> .
@prefix skos: <http://www.w3.org/2004/02/skos/core#> .
@prefix sw: <http://www.w3.org/2003/06/sw-vocab-status/ns#> .
@prefix vann: <http://purl.org/vocab/vann/> .
@prefix xsd: <http://www.w3.org/2001/XMLSchema#> .

sector-health-owl:AccessManagement a rdfs:Class,
        owl:Class,
        dpv-owl:Purpose ;
    dct:created "2024-12-01"^^xsd:date ;
    rdfs:isDefinedBy sector-health-owl: ;
    rdfs:subClassOf sector-health-owl:HealthcareServiceManagement ;
    sw:term_status "accepted"@en ;
    skos:definition "Purposes associated with managing access to infrastructure, resources, and services as part of healthcare"@en ;
    skos:prefLabel "Access Management"@en .

sector-health-owl:AppointmentScheduling a rdfs:Class,
        owl:Class,
        dpv-owl:Purpose ;
    dct:created "2024-12-01"^^xsd:date ;
    rdfs:isDefinedBy sector-health-owl: ;
    rdfs:subClassOf sector-health-owl:HealthcareServiceManagement ;
    sw:term_status "accepted"@en ;
    skos:definition "Purposes associated with scheduling appointments for use of healthcare services"@en ;
    skos:prefLabel "Appointment Scheduling"@en .

sector-health-owl:ConsultationManagement a rdfs:Class,
        owl:Class,
        dpv-owl:Purpose ;
    dct:created "2024-12-01"^^xsd:date ;
    rdfs:isDefinedBy sector-health-owl: ;
    rdfs:subClassOf sector-health-owl:ServiceProvision ;
    sw:term_status "accepted"@en ;
    skos:definition "Purposes associated with managing consultations as part of healthcare services"@en ;
    skos:prefLabel "Consultation Management"@en .

sector-health-owl:CrisisManagement a rdfs:Class,
        owl:Class,
        dpv-owl:Purpose ;
    dct:created "2024-12-01"^^xsd:date ;
    rdfs:isDefinedBy sector-health-owl: ;
    rdfs:subClassOf dpv-owl:ImproveHealthcare,
        sector-health-owl:HealthcareServiceManagement ;
    sw:term_status "accepted"@en ;
    skos:definition "Purposes associated with management of crisis situations in relation to healthcare services"@en ;
    skos:prefLabel "Crisis Management"@en .

sector-health-owl:DiagnosisManagement a rdfs:Class,
        owl:Class,
        dpv-owl:Purpose ;
    dct:created "2024-12-01"^^xsd:date ;
    rdfs:isDefinedBy sector-health-owl: ;
    rdfs:subClassOf sector-health-owl:ServiceProvision ;
    sw:term_status "accepted"@en ;
    skos:definition "Purposes associated with conducting and managing diagnosis as part of healthcare services"@en ;
    skos:prefLabel "Diagnosis Management"@en .

sector-health-owl:DiagnosticOptimisation a rdfs:Class,
        owl:Class,
        dpv-owl:Purpose ;
    dct:created "2024-12-01"^^xsd:date ;
    rdfs:isDefinedBy sector-health-owl: ;
    rdfs:subClassOf dpv-owl:ServiceOptimisation,
        sector-health-owl:Optimisation ;
    sw:term_status "accepted"@en ;
    skos:definition "Purposes associated with identifying optimisations related to use of diagnosis tools and processes as part of healthcare services"@en ;
    skos:prefLabel "Diagnostic Optimisation"@en .

sector-health-owl:DisasterReliefManagement a rdfs:Class,
        owl:Class,
        dpv-owl:Purpose ;
    dct:created "2024-12-01"^^xsd:date ;
    rdfs:isDefinedBy sector-health-owl: ;
    rdfs:subClassOf sector-health-owl:CrisisManagement ;
    sw:term_status "accepted"@en ;
    skos:definition "Purposes associated with management of disaster relief and related crisis situations in relation to healthcare services"@en ;
    skos:prefLabel "Disaster Relief Management"@en .

sector-health-owl:DiseasePreventionAwareness a rdfs:Class,
        owl:Class,
        dpv-owl:Purpose ;
    dct:created "2024-12-01"^^xsd:date ;
    rdfs:isDefinedBy sector-health-owl: ;
    rdfs:subClassOf sector-health-owl:PreventativeCareManagement ;
    sw:term_status "accepted"@en ;
    skos:definition "Purposes associated with management of disease prevention awareness as part of healthcare services"@en ;
    skos:prefLabel "Disease Prevention Awareness"@en .

sector-health-owl:EffectivenessAssessment a rdfs:Class,
        owl:Class,
        dpv-owl:Purpose ;
    dct:created "2024-12-01"^^xsd:date ;
    rdfs:isDefinedBy sector-health-owl: ;
    rdfs:subClassOf sector-health-owl:ResearchDevelopment ;
    sw:term_status "accepted"@en ;
    skos:definition "Purposes associated with assessing the effectiveness of healthcare infrastructure and services"@en ;
    skos:prefLabel "Effectiveness Assessment"@en .

sector-health-owl:ElectronicRecordsManagement a rdfs:Class,
        owl:Class,
        dpv-owl:Purpose ;
    dct:created "2024-12-01"^^xsd:date ;
    rdfs:isDefinedBy sector-health-owl: ;
    rdfs:subClassOf sector-health-owl:PatientInformationManagement ;
    sw:term_status "accepted"@en ;
    skos:definition "Purposes associated with management of patient information in electronic forms for healthcare services"@en ;
    skos:prefLabel "Electronic Records Management"@en .

sector-health-owl:EligibilityAssessment a rdfs:Class,
        owl:Class,
        dpv-owl:Purpose ;
    dct:created "2024-12-01"^^xsd:date ;
    rdfs:isDefinedBy sector-health-owl: ;
    rdfs:subClassOf sector-health-owl:HealthcareServiceManagement ;
    sw:term_status "accepted"@en ;
    skos:definition "Purposes associated with assessment of eligibility to receive or continue to receive healthcare services"@en ;
    skos:prefLabel "Eligibility Assessment"@en .

sector-health-owl:EmergencyCareCommunication a rdfs:Class,
        owl:Class,
        dpv-owl:Purpose ;
    dct:created "2024-12-01"^^xsd:date ;
    rdfs:isDefinedBy sector-health-owl: ;
    rdfs:subClassOf sector-health-owl:EmergencyCareManagement ;
    sw:term_status "accepted"@en ;
    skos:definition "Purposes associated with management of communication for emergency care as part of healthcare services"@en ;
    skos:prefLabel "Emergency Care Communication"@en .

sector-health-owl:EmergencyCareDispatch a rdfs:Class,
        owl:Class,
        dpv-owl:Purpose ;
    dct:created "2024-12-01"^^xsd:date ;
    rdfs:isDefinedBy sector-health-owl: ;
    rdfs:subClassOf sector-health-owl:EmergencyCareManagement ;
    sw:term_status "accepted"@en ;
    skos:definition "Purposes associated with management of emergency care dispatch as part of healthcare services"@en ;
    skos:prefLabel "Emergency Care Dispatch"@en .

sector-health-owl:EmergencyCareEligibilityAssessment a rdfs:Class,
        owl:Class,
        dpv-owl:Purpose ;
    dct:created "2024-12-01"^^xsd:date ;
    rdfs:isDefinedBy sector-health-owl: ;
    rdfs:subClassOf sector-health-owl:EmergencyCareManagement ;
    sw:term_status "accepted"@en ;
    skos:definition "Purposes associated with assessment of eligibility to receive or continue to receive emergency care as part of healthcare services"@en ;
    skos:prefLabel "Emergency Care Eligibility Assessment"@en .

sector-health-owl:EmergencyCareManagement a rdfs:Class,
        owl:Class,
        dpv-owl:Purpose ;
    dct:created "2024-12-01"^^xsd:date ;
    rdfs:isDefinedBy sector-health-owl: ;
    rdfs:subClassOf sector-health-owl:HealthcareServiceManagement ;
    sw:term_status "accepted"@en ;
    skos:definition "Purposes associated with management of emergency care as part of healthcare services"@en ;
    skos:prefLabel "Emergency Care Management"@en .

sector-health-owl:EmergencyCareTriage a rdfs:Class,
        owl:Class,
        dpv-owl:Purpose ;
    dct:created "2024-12-01"^^xsd:date ;
    rdfs:isDefinedBy sector-health-owl: ;
    rdfs:subClassOf sector-health-owl:EmergencyCareManagement ;
    sw:term_status "accepted"@en ;
    skos:definition "Purposes associated with management of prioritisation and other triage processes as part of emergency care in healthcare services"@en ;
    skos:prefLabel "Emergency Care Triage"@en .

sector-health-owl:FitnessNutritionAwareness a rdfs:Class,
        owl:Class,
        dpv-owl:Purpose ;
    dct:created "2024-12-01"^^xsd:date ;
    rdfs:isDefinedBy sector-health-owl: ;
    rdfs:subClassOf sector-health-owl:PreventativeCareManagement ;
    sw:term_status "accepted"@en ;
    skos:definition "Purposes associated with management of fitness and nutrition awareness as part of healthcare services"@en ;
    skos:prefLabel "Fitness Nutrition Awareness"@en .

sector-health-owl:FraudPreventionDetection a rdfs:Class,
        owl:Class,
        dpv-owl:Purpose ;
    dct:created "2024-12-01"^^xsd:date ;
    rdfs:isDefinedBy sector-health-owl: ;
    rdfs:subClassOf dpv-owl:FraudPreventionAndDetection,
        sector-health-owl:SecurityManagement ;
    sw:term_status "accepted"@en ;
    skos:definition "Purposes associated with fraud prevention and detection in relation to healthcare services"@en ;
    skos:prefLabel "Fraud Prevention Detection"@en .

sector-health-owl:GeneticConditionDiagnosis a rdfs:Class,
        owl:Class,
        dpv-owl:Purpose ;
    dct:created "2024-12-01"^^xsd:date ;
    rdfs:isDefinedBy sector-health-owl: ;
    rdfs:subClassOf sector-health-owl:DiagnosisManagement ;
    sw:term_status "accepted"@en ;
    skos:definition "Purposes associated with conducting and managing genetic diagnosis as part of healthcare services"@en ;
    skos:prefLabel "Genetic Condition Diagnosis"@en .

sector-health-owl:HealthInequalityAnalysis a rdfs:Class,
        owl:Class,
        dpv-owl:Purpose ;
    dct:created "2024-12-01"^^xsd:date ;
    rdfs:isDefinedBy sector-health-owl: ;
    rdfs:subClassOf sector-health-owl:ResearchDevelopment ;
    sw:term_status "accepted"@en ;
    skos:definition "Purposes associated with detecting, analysing, and identifying ways to mitigate inequality in provision and use of healthcare services"@en ;
    skos:prefLabel "Health Inequality Analysis"@en .

sector-health-owl:HealthInsuranceManagement a rdfs:Class,
        owl:Class,
        dpv-owl:Purpose ;
    dct:created "2024-12-01"^^xsd:date ;
    rdfs:isDefinedBy sector-health-owl: ;
    rdfs:subClassOf sector-health-owl:InsuranceManagement ;
    sw:term_status "accepted"@en ;
    skos:definition "Purposes associated with managing health insurance as part of healthcare services"@en ;
    skos:prefLabel "Health Insurance Management"@en .

sector-health-owl:HealthTrendAnalysis a rdfs:Class,
        owl:Class,
        dpv-owl:Purpose ;
    dct:created "2024-12-01"^^xsd:date ;
    rdfs:isDefinedBy sector-health-owl: ;
    rdfs:subClassOf sector-health-owl:ResearchDevelopment ;
    sw:term_status "accepted"@en ;
    skos:definition "Purposes associated with analysing trends in public health and safety"@en ;
    skos:prefLabel "Health Trend Analysis"@en .

sector-health-owl:HealthcareManagement a rdfs:Class,
        owl:Class,
        dpv-owl:Purpose ;
    dct:created "2024-12-01"^^xsd:date ;
    rdfs:isDefinedBy sector-health-owl: ;
    rdfs:subClassOf dpv-owl:Purpose ;
    sw:term_status "accepted"@en ;
    skos:definition "Purposes associated with management of healthcare infrastructure and services"@en ;
    skos:prefLabel "Healthcare Management"@en .

sector-health-owl:HealthcareServiceManagement a rdfs:Class,
        owl:Class,
        dpv-owl:Purpose ;
    dct:created "2024-12-01"^^xsd:date ;
    rdfs:isDefinedBy sector-health-owl: ;
    rdfs:subClassOf sector-health-owl:HealthcareManagement ;
    sw:term_status "accepted"@en ;
    skos:definition "Purposes associated with management of healthcare services"@en ;
    skos:prefLabel "Healthcare Service Management"@en .

sector-health-owl:IdentityFraudManagement a rdfs:Class,
        owl:Class,
        dpv-owl:Purpose ;
    dct:created "2024-12-01"^^xsd:date ;
    rdfs:isDefinedBy sector-health-owl: ;
    rdfs:subClassOf sector-health-owl:FraudPreventionDetection ;
    sw:term_status "accepted"@en ;
    skos:definition "Purposes associated with identity prevention and detection in relation to healthcare services"@en ;
    skos:prefLabel "Identity Fraud Management"@en .

sector-health-owl:InsuranceClaimFraudManagement a rdfs:Class,
        owl:Class,
        dpv-owl:Purpose ;
    dct:created "2024-12-01"^^xsd:date ;
    rdfs:isDefinedBy sector-health-owl: ;
    rdfs:subClassOf sector-health-owl:FraudPreventionDetection ;
    sw:term_status "accepted"@en ;
    skos:definition "Purposes associated with insurance fraud prevention and detection in relation to healthcare services"@en ;
    skos:prefLabel "Insurance Claim Fraud Management"@en .

sector-health-owl:InsuranceManagement a rdfs:Class,
        owl:Class,
        dpv-owl:Purpose ;
    dct:created "2024-12-01"^^xsd:date ;
    rdfs:isDefinedBy sector-health-owl: ;
    rdfs:subClassOf sector-health-owl:HealthcareManagement ;
    sw:term_status "accepted"@en ;
    skos:definition "Purposes associated with management of insurance as part of providing healthcare services"@en ;
    skos:prefLabel "Insurance Management"@en .

sector-health-owl:LifeInsuranceManagement a rdfs:Class,
        owl:Class,
        dpv-owl:Purpose ;
    dct:created "2024-12-01"^^xsd:date ;
    rdfs:isDefinedBy sector-health-owl: ;
    rdfs:subClassOf sector-health-owl:InsuranceManagement ;
    sw:term_status "accepted"@en ;
    skos:definition "Purposes associated with managing life insurance as part of healthcare services"@en ;
    skos:prefLabel "Life Insurance Management"@en .

sector-health-owl:MedicalConditionDiagnosis a rdfs:Class,
        owl:Class,
        dpv-owl:Purpose ;
    dct:created "2024-12-01"^^xsd:date ;
    rdfs:isDefinedBy sector-health-owl: ;
    rdfs:subClassOf sector-health-owl:DiagnosisManagement ;
    sw:term_status "accepted"@en ;
    skos:definition "Purposes associated with conducting and managing medical diagnosis as part of healthcare services"@en ;
    skos:prefLabel "Medical Condition Diagnosis"@en .

sector-health-owl:MedicalResourceOptimisation a rdfs:Class,
        owl:Class,
        dpv-owl:Purpose ;
    dct:created "2024-12-01"^^xsd:date ;
    rdfs:isDefinedBy sector-health-owl: ;
    rdfs:subClassOf sector-health-owl:Optimisation ;
    sw:term_status "accepted"@en ;
    skos:definition "Purposes associated with identifying optimisations related to use of medical resources as part of healthcare services"@en ;
    skos:prefLabel "Medical Resource Optimisation"@en .

sector-health-owl:MentalHealthAwareness a rdfs:Class,
        owl:Class,
        dpv-owl:Purpose ;
    dct:created "2024-12-01"^^xsd:date ;
    rdfs:isDefinedBy sector-health-owl: ;
    rdfs:subClassOf sector-health-owl:PreventativeCareManagement ;
    sw:term_status "accepted"@en ;
    skos:definition "Purposes associated with management of mental health awareness as part of healthcare services"@en ;
    skos:prefLabel "Mental Health Awareness"@en .

sector-health-owl:MentalHealthConditionDiagnosis a rdfs:Class,
        owl:Class,
        dpv-owl:Purpose ;
    dct:created "2024-12-01"^^xsd:date ;
    rdfs:isDefinedBy sector-health-owl: ;
    rdfs:subClassOf sector-health-owl:DiagnosisManagement ;
    sw:term_status "accepted"@en ;
    skos:definition "Purposes associated with conducting and managing mental health diagnosis as part of healthcare services"@en ;
    skos:prefLabel "Mental Health Condition Diagnosis"@en .

sector-health-owl:Optimisation a rdfs:Class,
        owl:Class,
        dpv-owl:Purpose ;
    dct:created "2024-12-01"^^xsd:date ;
    rdfs:isDefinedBy sector-health-owl: ;
    rdfs:subClassOf dpv-owl:ImproveHealthcare,
        sector-health-owl:HealthcareManagement ;
    sw:term_status "accepted"@en ;
    skos:definition "Purposes associated with identifying optimisations to use and provision of healthcare services"@en ;
    skos:prefLabel "Optimisation"@en .

sector-health-owl:PandemicResponseManagement a rdfs:Class,
        owl:Class,
        dpv-owl:Purpose ;
    dct:created "2024-12-01"^^xsd:date ;
    rdfs:isDefinedBy sector-health-owl: ;
    rdfs:subClassOf sector-health-owl:CrisisManagement ;
    sw:term_status "accepted"@en ;
    skos:definition "Purposes associated with management of pandemics and related crisis situations in relation to healthcare services"@en ;
    skos:prefLabel "Pandemic Response Management"@en .

sector-health-owl:PatientChronicConditionMonitoring a rdfs:Class,
        owl:Class,
        dpv-owl:Purpose ;
    dct:created "2024-12-01"^^xsd:date ;
    rdfs:isDefinedBy sector-health-owl: ;
    rdfs:subClassOf sector-health-owl:PatientMonitoring ;
    sw:term_status "accepted"@en ;
    skos:definition "Purposes associated with monitoring of patients with chronic conditions for health and safety as part of healthcare services"@en ;
    skos:prefLabel "Patient Chronic Condition Monitoring"@en .

sector-health-owl:PatientConsentManagement a rdfs:Class,
        owl:Class,
        dpv-owl:Purpose ;
    dct:created "2024-12-01"^^xsd:date ;
    rdfs:isDefinedBy sector-health-owl: ;
    rdfs:subClassOf sector-health-owl:PatientInformationManagement ;
    sw:term_status "accepted"@en ;
    skos:definition "Purposes associated with management of consent from or related to patients in relation to healthcare services"@en ;
    skos:prefLabel "Patient Consent Management"@en .

sector-health-owl:PatientInformationManagement a rdfs:Class,
        owl:Class,
        dpv-owl:Purpose ;
    dct:created "2024-12-01"^^xsd:date ;
    rdfs:isDefinedBy sector-health-owl: ;
    rdfs:subClassOf sector-health-owl:ResourceManagement ;
    sw:term_status "accepted"@en ;
    skos:definition "Purposes associated with management of patient information in relation to healthcare services"@en ;
    skos:prefLabel "Patient Information Management"@en .

sector-health-owl:PatientIntensiveCareMonitoring a rdfs:Class,
        owl:Class,
        dpv-owl:Purpose ;
    dct:created "2024-12-01"^^xsd:date ;
    rdfs:isDefinedBy sector-health-owl: ;
    rdfs:subClassOf sector-health-owl:PatientMonitoring ;
    sw:term_status "accepted"@en ;
    skos:definition "Purposes associated with monitoring of patients in intensive care as part of healthcare services"@en ;
    skos:prefLabel "Patient Intensive Care Monitoring"@en .

sector-health-owl:PatientMonitoring a rdfs:Class,
        owl:Class,
        dpv-owl:Purpose ;
    dct:created "2024-12-01"^^xsd:date ;
    rdfs:isDefinedBy sector-health-owl: ;
    rdfs:subClassOf sector-health-owl:ServiceProvision ;
    sw:term_status "accepted"@en ;
    skos:definition "Purposes associated with monitoring of patients for treatment and safety as part of healthcare services"@en ;
    skos:prefLabel "Patient Monitoring"@en .

sector-health-owl:PatientPostTreatmentMonitoring a rdfs:Class,
        owl:Class,
        dpv-owl:Purpose ;
    dct:created "2024-12-01"^^xsd:date ;
    rdfs:isDefinedBy sector-health-owl: ;
    rdfs:subClassOf sector-health-owl:PatientMonitoring ;
    sw:term_status "accepted"@en ;
    skos:definition "Purposes associated with monitoring of patients post-treatment for health and safety as part of healthcare services"@en ;
    skos:prefLabel "Patient Post Treatment Monitoring"@en .

sector-health-owl:PatientRemoteMonitoring a rdfs:Class,
        owl:Class,
        dpv-owl:Purpose ;
    dct:created "2024-12-01"^^xsd:date ;
    rdfs:isDefinedBy sector-health-owl: ;
    rdfs:subClassOf sector-health-owl:PatientMonitoring ;
    sw:term_status "accepted"@en ;
    skos:definition "Purposes associated with remote monitoring of patients for treatment and safety as part of healthcare services"@en ;
    skos:prefLabel "Patient Remote Monitoring"@en .

sector-health-owl:PatientTreatmentEffectivenessMonitoring a rdfs:Class,
        owl:Class,
        dpv-owl:Purpose ;
    dct:created "2024-12-01"^^xsd:date ;
    rdfs:isDefinedBy sector-health-owl: ;
    rdfs:subClassOf sector-health-owl:PatientMonitoring ;
    sw:term_status "accepted"@en ;
    skos:definition "Purposes associated with monitoring of treatment effectiveness as part of healthcare services"@en ;
    skos:prefLabel "Patient Treatment Effectiveness Monitoring"@en .

sector-health-owl:PatientTreatmentOutcomeAnalysis a rdfs:Class,
        owl:Class,
        dpv-owl:Purpose ;
    dct:created "2024-12-01"^^xsd:date ;
    rdfs:isDefinedBy sector-health-owl: ;
    rdfs:subClassOf sector-health-owl:PatientMonitoring ;
    sw:term_status "accepted"@en ;
    skos:definition "Purposes associated with analysis of patient treatment outcomes as part of healthcare services"@en ;
    skos:prefLabel "Patient Treatment Outcome Analysis"@en .

sector-health-owl:PopulationHealthAnalysis a rdfs:Class,
        owl:Class,
        dpv-owl:Purpose ;
    dct:created "2024-12-01"^^xsd:date ;
    rdfs:isDefinedBy sector-health-owl: ;
    rdfs:subClassOf sector-health-owl:ResearchDevelopment ;
    sw:term_status "accepted"@en ;
    skos:definition "Purposes associated with analysing trends and outcomes in a specific population or group of people regarding health and safety"@en ;
    skos:prefLabel "Population Health Analysis"@en .

sector-health-owl:PredictiveHealthRiskAnalysis a rdfs:Class,
        owl:Class,
        dpv-owl:Purpose ;
    dct:created "2024-12-01"^^xsd:date ;
    rdfs:isDefinedBy sector-health-owl: ;
    rdfs:subClassOf sector-health-owl:ResearchDevelopment ;
    sw:term_status "accepted"@en ;
    skos:definition "Purposes associated with analysing and predicting risks to public health and safety"@en ;
    skos:prefLabel "Predictive Health Risk Analysis"@en .

sector-health-owl:PreventativeCareManagement a rdfs:Class,
        owl:Class,
        dpv-owl:Purpose ;
    dct:created "2024-12-01"^^xsd:date ;
    rdfs:isDefinedBy sector-health-owl: ;
    rdfs:subClassOf dpv-owl:ImproveHealthcare,
        sector-health-owl:HealthcareServiceManagement ;
    sw:term_status "accepted"@en ;
    skos:definition "Purposes associated with management of preventative care as part of healthcare services"@en ;
    skos:prefLabel "Preventative Care Management"@en .

sector-health-owl:PrimaryCareManagement a rdfs:Class,
        owl:Class,
        dpv-owl:Purpose ;
    dct:created "2024-12-01"^^xsd:date ;
    rdfs:isDefinedBy sector-health-owl: ;
    rdfs:subClassOf sector-health-owl:HealthcareServiceManagement ;
    sw:term_status "accepted"@en ;
    skos:definition "Purposes associated with management of primary healthcare services"@en ;
    skos:prefLabel "Primary Care Management"@en .

sector-health-owl:ProvidersDataSharing a rdfs:Class,
        owl:Class,
        dpv-owl:Purpose ;
    dct:created "2024-12-01"^^xsd:date ;
    rdfs:isDefinedBy sector-health-owl: ;
    rdfs:subClassOf sector-health-owl:HealthcareServiceManagement ;
    sw:term_status "accepted"@en ;
    skos:definition "Purposes associated with sharing of patient information between healthcare providers, such as between hospitals treating the same patient"@en ;
    skos:prefLabel "Providers Data Sharing"@en .

sector-health-owl:PublicHealthMonitoring a rdfs:Class,
        owl:Class,
        dpv-owl:Purpose ;
    dct:created "2024-12-01"^^xsd:date ;
    rdfs:isDefinedBy sector-health-owl: ;
    rdfs:subClassOf sector-health-owl:PreventativeCareManagement ;
    sw:term_status "accepted"@en ;
    skos:definition "Purposes associated with monitoring of public health as part of healthcare services"@en ;
    skos:prefLabel "Public Health Monitoring"@en .

sector-health-owl:ReferralManagement a rdfs:Class,
        owl:Class,
        dpv-owl:Purpose ;
    dct:created "2024-12-01"^^xsd:date ;
    rdfs:isDefinedBy sector-health-owl: ;
    rdfs:subClassOf sector-health-owl:HealthcareServiceManagement ;
    sw:term_status "accepted"@en ;
    skos:definition "Purposes associated with management of referrals as part of healthcare services"@en ;
    skos:prefLabel "Referral Management"@en .

sector-health-owl:ResearchDevelopment a rdfs:Class,
        owl:Class,
        dpv-owl:Purpose ;
    dct:created "2024-12-01"^^xsd:date ;
    rdfs:isDefinedBy sector-health-owl: ;
    rdfs:subClassOf dpv-owl:ImproveHealthcare,
        dpv-owl:ResearchAndDevelopment,
        sector-health-owl:HealthcareManagement ;
    sw:term_status "accepted"@en ;
    skos:definition "Purposes associated with research and development regarding healthcare services"@en ;
    skos:prefLabel "Research Development"@en .

sector-health-owl:ResourceManagement a rdfs:Class,
        owl:Class,
        dpv-owl:Purpose ;
    dct:created "2024-12-01"^^xsd:date ;
    rdfs:isDefinedBy sector-health-owl: ;
    rdfs:subClassOf sector-health-owl:HealthcareManagement ;
    sw:term_status "accepted"@en ;
    skos:definition "Purposes associated with management of resources related to healthcare services"@en ;
    skos:prefLabel "Resource Management"@en .

sector-health-owl:SecurityManagement a rdfs:Class,
        owl:Class,
        dpv-owl:Purpose ;
    dct:created "2024-12-01"^^xsd:date ;
    rdfs:isDefinedBy sector-health-owl: ;
    rdfs:subClassOf dpv-owl:OrganisationRiskManagement,
        sector-health-owl:HealthcareManagement ;
    sw:term_status "accepted"@en ;
    skos:definition "Purposes associated with management of security in relation to healthcare services"@en ;
    skos:prefLabel "Security Management"@en .

sector-health-owl:ServiceBillingFraudManagement a rdfs:Class,
        owl:Class,
        dpv-owl:Purpose ;
    dct:created "2024-12-01"^^xsd:date ;
    rdfs:isDefinedBy sector-health-owl: ;
    rdfs:subClassOf sector-health-owl:FraudPreventionDetection ;
    sw:term_status "accepted"@en ;
    skos:definition "Purposes associated with billing prevention and detection in relation to healthcare services"@en ;
    skos:prefLabel "Service Billing Fraud Management"@en .

sector-health-owl:ServiceProvision a rdfs:Class,
        owl:Class,
        dpv-owl:Purpose ;
    dct:created "2024-12-01"^^xsd:date ;
    rdfs:isDefinedBy sector-health-owl: ;
    rdfs:subClassOf dpv-owl:ServiceProvision,
        sector-health-owl:HealthcareServiceManagement ;
    sw:term_status "accepted"@en ;
    skos:definition "Purposes associated with provision of healthcare services"@en ;
    skos:prefLabel "Service Provision"@en .

sector-health-owl:SpecialisedCareManagement a rdfs:Class,
        owl:Class,
        dpv-owl:Purpose ;
    dct:created "2024-12-01"^^xsd:date ;
    rdfs:isDefinedBy sector-health-owl: ;
    rdfs:subClassOf sector-health-owl:HealthcareServiceManagement ;
    sw:term_status "accepted"@en ;
    skos:definition "Purposes associated with management of specialised healthcare services"@en ;
    skos:prefLabel "Specialised Care Management"@en .

sector-health-owl:TreatmentOptimisation a rdfs:Class,
        owl:Class,
        dpv-owl:Purpose ;
    dct:created "2024-12-01"^^xsd:date ;
    rdfs:isDefinedBy sector-health-owl: ;
    rdfs:subClassOf dpv-owl:ServiceOptimisation,
        sector-health-owl:Optimisation ;
    sw:term_status "accepted"@en ;
    skos:definition "Purposes associated with identifying optimisations related to use of treatments and related processes as part of healthcare services"@en ;
    skos:prefLabel "Treatment Optimisation"@en .

sector-health-owl:VaccinationManagement a rdfs:Class,
        owl:Class,
        dpv-owl:Purpose ;
    dct:created "2024-12-01"^^xsd:date ;
    rdfs:isDefinedBy sector-health-owl: ;
    rdfs:subClassOf sector-health-owl:PreventativeCareManagement ;
    sw:term_status "accepted"@en ;
    skos:definition "Purposes associated with management of vaccinations as part of healthcare services"@en ;
    skos:prefLabel "Vaccination Management"@en .

sector-health-owl:WorkforceManagement a rdfs:Class,
        owl:Class,
        dpv-owl:Purpose ;
    dct:created "2024-12-01"^^xsd:date ;
    rdfs:isDefinedBy sector-health-owl: ;
    rdfs:subClassOf sector-health-owl:HealthcareManagement ;
    sw:term_status "accepted"@en ;
    skos:definition "Purposes associated with management of workforce involved in provision of healthcare services"@en ;
    skos:prefLabel "Workforce Management"@en .

sector-health-owl:serialisation-html a profile:ResourceDescriptor ;
    dct:conformsTo <https://www.w3.org/TR/html/> ;
    dct:format <https://www.iana.org/assignments/media-types/text/html> ;
    dct:title "Health Sector Concepts - HTML serialisation" ;
    profile:hasArtifact <https://w3id.org/dpv/sector/health/sector-health-owl.html> ;
    profile:hasRole role:specification .

sector-health-owl:serialisation-jsonld a profile:ResourceDescriptor ;
    dct:conformsTo <https://www.w3.org/TR/json-ld11/> ;
    dct:format <https://www.iana.org/assignments/media-types/application/ld+json> ;
    dct:title "Health Sector Concepts - JSON-LD serialisation" ;
    profile:hasArtifact <https://w3id.org/dpv/sector/health/sector-health-owl.jsonld> ;
    profile:hasRole role:vocabulary .

sector-health-owl:serialisation-n3 a profile:ResourceDescriptor ;
    dct:conformsTo <https://www.w3.org/TeamSubmission/n3/> ;
    dct:format <https://www.iana.org/assignments/media-types/text/n3> ;
    dct:title "Health Sector Concepts - N3 serialisation" ;
    profile:hasArtifact <https://w3id.org/dpv/sector/health/sector-health-owl.n3> ;
    profile:hasRole role:vocabulary .

sector-health-owl:serialisation-rdf a profile:ResourceDescriptor ;
    dct:conformsTo rdf: ;
    dct:format <https://www.iana.org/assignments/media-types/application/rdf+xml> ;
    dct:title "Health Sector Concepts - RDF/XML serialisation" ;
    profile:hasArtifact <https://w3id.org/dpv/sector/health/sector-health-owl.rdf> ;
    profile:hasRole role:vocabulary .

sector-health-owl:serialisation-ttl a profile:ResourceDescriptor ;
    dct:conformsTo <https://www.w3.org/TR/turtle/> ;
    dct:format <https://www.iana.org/assignments/media-types/text/turtle> ;
    dct:title "Health Sector Concepts - Turtle serialisation" ;
    profile:hasArtifact <https://w3id.org/dpv/sector/health/sector-health-owl.ttl> ;
    profile:hasRole role:vocabulary .

<https://w3id.org/dpv/examples> a profile:ResourceDescriptor ;
    dct:conformsTo <https://www.w3.org/TR/html/> ;
    dct:format <https://www.iana.org/assignments/media-types/text/html> ;
    dct:title "Examples" ;
    profile:hasArtifact <https://w3id.org/dpv/examples> ;
    profile:hasRole role:guidance .

<https://w3id.org/dpv/guides> a profile:ResourceDescriptor ;
    dct:conformsTo <https://www.w3.org/TR/html/> ;
    dct:format <https://www.iana.org/assignments/media-types/text/html> ;
    dct:title "Guides for Data Privacy Vocabulary" ;
    profile:hasArtifact <https://w3id.org/dpv/guides> ;
    profile:hasRole role:guidance .

<https://w3id.org/dpv/primer> a profile:ResourceDescriptor ;
    dct:conformsTo <https://www.w3.org/TR/html/> ;
    dct:format <https://www.iana.org/assignments/media-types/text/html> ;
    dct:title "Primer for Data Privacy Vocabulary" ;
    profile:hasArtifact <https://w3id.org/dpv/primer> ;
    profile:hasRole role:guidance .

sector-health-owl: a owl:Ontology,
        profile:Profile ;
    dct:bibliographicCitation "Harshvardhan J. Pandit, Beatriz Esteves, Georg P. Krog, Paul Ryan, Delaram Golpayegani, Julian Flake (2025) Data Privacy Vocabulary (DPV) – Version 2.0. In: Demartini, G., et al. The Semantic Web – ISWC 2024. ISWC 2024. Lecture Notes in Computer Science, vol 15233. Springer, Cham. https://doi.org/10.1007/978-3-031-77847-6_10" ;
    dct:conformsTo <http://www.w3.org/2002/07/owl>,
        "http://www.w3.org/2000/01/rdf-schema",
        "http://www.w3.org/2004/02/skos/core" ;
    dct:created "2024-12-01"@en ;
    dct:creator [ a dct:Agent,
                foaf:Person ;
            scoro:hasORCID "0000-0002-5068-3714" ;
            org:memberOf [ a foaf:Organization ;
                    foaf:name "AI Accountability Lab (AIAL), Trinity College Dublin" ] ;
            foaf:homepage "https://harshp.com/" ;
            foaf:name "Harshvardhan J. Pandit" ] ;
    dct:description "Extension to the Data Privacy Vocabulary (DPV) providing concepts for the health sector"@en ;
    dct:hasVersion sector-health-owl: ;
    dct:identifier "https://w3id.org/dpv/sector/health" ;
    dct:issued "2024-12-01"@en ;
    dct:license <https://www.w3.org/copyright/document-license-2023/> ;
    dct:modified "2025-08-01"@en ;
    dct:publisher <https://www.w3.org/> ;
    dct:source <https://www.w3.org/groups/cg/dpvcg/> ;
    dct:title "Health Sector Concepts"@en ;
    bibo:doi "10.5281/zenodo.12505841" ;
    bibo:status "http://purl.org/ontology/bibo/status/draft" ;
    vann:preferredNamespacePrefix "sector-health" ;
    vann:preferredNamespaceUri "https://w3id.org/dpv/sector/health#" ;
    rdfs:Label "SECTOR-HEALTH"@en ;
    owl:versionIRI <https://w3id.org/dpv/2.2/sector/health/owl#> ;
    owl:versionInfo "2.2" ;
    profile:hasResource <https://w3id.org/dpv/examples>,
        <https://w3id.org/dpv/guides>,
        <https://w3id.org/dpv/primer>,
        sector-health-owl:serialisation-html,
        sector-health-owl:serialisation-jsonld,
        sector-health-owl:serialisation-n3,
        sector-health-owl:serialisation-rdf,
        sector-health-owl:serialisation-ttl ;
    profile:isProfileOf <http://www.w3.org/2002/07/owl>,
        <https://w3id.org/dpv/owl>,
        sector-health-owl: ;
    foaf:logo <https://w3id.org/dpv/media/logo.png> ;
    schema:version "2.2" .

