@prefix bibo: <http://purl.org/ontology/bibo/> .
@prefix dcam: <http://purl.org/dc/dcam/> .
@prefix dct: <http://purl.org/dc/terms/> .
@prefix dpv-owl: <https://w3id.org/dpv/owl#> .
@prefix eu-dga-owl: <https://w3id.org/dpv/legal/eu/dga/owl#> .
@prefix foaf: <http://xmlns.com/foaf/0.1/> .
@prefix org: <http://www.w3.org/ns/org#> .
@prefix owl: <http://www.w3.org/2002/07/owl#> .
@prefix profile: <http://www.w3.org/ns/dx/prof/> .
@prefix rdf: <http://www.w3.org/1999/02/22-rdf-syntax-ns#> .
@prefix rdfs: <http://www.w3.org/2000/01/rdf-schema#> .
@prefix risk-owl: <https://w3id.org/dpv/risk/owl#> .
@prefix role: <http://www.w3.org/ns/dx/prof/role/> .
@prefix schema: <https://schema.org/> .
@prefix scoro: <http://purl.org/spar/scoro/> .
@prefix skos: <http://www.w3.org/2004/02/skos/core#> .
@prefix sw: <http://www.w3.org/2003/06/sw-vocab-status/ns#> .
@prefix vann: <http://purl.org/vocab/vann/> .
@prefix xsd: <http://www.w3.org/2001/XMLSchema#> .

eu-dga-owl:A12-e-Exchange-Approval a rdfs:Class,
        owl:Class,
        dpv-owl:LegalBasis ;
    dct:contributor _:N458008bc6195484e9cc557f70eabda31 ;
    dct:created "2024-02-14"^^xsd:date ;
    dct:source [ a schema:WebPage ;
            schema:name "DGA 12.e" ;
            schema:url "https://eur-lex.europa.eu/eli/reg/2022/868/art_12/par_e/oj" ] ;
    rdfs:isDefinedBy eu-dga-owl: ;
    rdfs:subClassOf dpv-owl:LegalBasis ;
    sw:term_status "accepted"@en ;
    skos:definition "Explicit request or approval of the data subject or data holder to utilise additional specific tools for the purposes of facilitating exchange of data"@en ;
    skos:prefLabel "Art 12(e) Data Exchange Approval"@en .

eu-dga-owl:A2-6-Permission a rdfs:Class,
        owl:Class,
        dpv-owl:LegalBasis ;
    dct:contributor _:N458008bc6195484e9cc557f70eabda31 ;
    dct:created "2024-02-14"^^xsd:date ;
    dct:source [ a schema:WebPage ;
            schema:name "DGA 2.6" ;
            schema:url "https://eur-lex.europa.eu/eli/reg/2022/868/art_2/par_6/oj" ] ;
    rdfs:isDefinedBy eu-dga-owl: ;
    rdfs:subClassOf dpv-owl:LegalBasis ;
    sw:term_status "accepted"@en ;
    skos:definition "The legal basis justifying processing of non-personal data based on the permission of an entity"@en ;
    skos:prefLabel "Art 2(6) Permission"@en .

eu-dga-owl:A27 a rdfs:Class,
        owl:Class,
        dpv-owl:Right ;
    dct:contributor _:N0a43dd9ea5e94fe695d8b7df8802cfdd,
        _:N458008bc6195484e9cc557f70eabda31 ;
    dct:created "2024-02-14"^^xsd:date ;
    dct:modified "2024-12-17"^^xsd:date ;
    dct:source "DGA 27"@en ;
    rdfs:isDefinedBy eu-dga-owl: ;
    rdfs:subClassOf dpv-owl:Right ;
    sw:term_status "modified"@en ;
    skos:definition "Right of natural and legal persons to lodge a complaint"@en ;
    skos:prefLabel "A27 Right to Lodge Complaint"@en .

eu-dga-owl:A27-Impact a rdfs:Class,
        owl:Class,
        dpv-owl:RiskConcept,
        risk-owl:PotentialConsequence,
        risk-owl:PotentialImpact,
        risk-owl:PotentialRisk ;
    dct:contributor _:N0a43dd9ea5e94fe695d8b7df8802cfdd ;
    dct:created "2024-12-17"^^xsd:date ;
    dct:source "DGA 27"@en ;
    rdfs:isDefinedBy eu-dga-owl: ;
    rdfs:subClassOf eu-dga-owl:DGARightsImpact ;
    sw:term_status "accepted"@en ;
    skos:definition "Something that acts as or is considered as an impact on Right of natural and legal persons to lodge a complaint"@en ;
    skos:prefLabel "Impact on A27 Right to Lodge Complaint"@en .

eu-dga-owl:A28 a rdfs:Class,
        owl:Class,
        dpv-owl:Right ;
    dct:contributor _:N0a43dd9ea5e94fe695d8b7df8802cfdd ;
    dct:created "2024-12-17"^^xsd:date ;
    dct:source "DGA 28"@en ;
    rdfs:isDefinedBy eu-dga-owl: ;
    rdfs:subClassOf dpv-owl:Right ;
    sw:term_status "accepted"@en ;
    skos:definition "Right of affected natural and legal persons to an effective judicial remedy"@en ;
    skos:prefLabel "A28 Right to an effective judicial remedy"@en ;
    skos:scopeNote "The right is scoped to legally binding decisions referred to in Article 14 taken by the competent authorities for data intermediation services in the management, control and enforcement of the notification regime for data intermediation services providers and legally binding decisions referred to in Articles 19 and 24 taken by the competent authorities for the registration of data altruism organisations in the monitoring of recognised data altruism organisations"@en .

eu-dga-owl:A28-3 a rdfs:Class,
        owl:Class,
        dpv-owl:Right ;
    dct:contributor _:N0a43dd9ea5e94fe695d8b7df8802cfdd,
        _:N458008bc6195484e9cc557f70eabda31 ;
    dct:created "2024-02-14"^^xsd:date ;
    dct:modified "2024-12-17"^^xsd:date ;
    dct:source "DGA 28.3"@en ;
    rdfs:isDefinedBy eu-dga-owl: ;
    rdfs:subClassOf eu-dga-owl:A28 ;
    sw:term_status "modified"@en ;
    skos:definition "Right of natural and legal persons to get a review by an impartial body with the appropriate expertise"@en ;
    skos:prefLabel "A28-3 Right to Impartial Review"@en .

eu-dga-owl:A28-3-Impact a rdfs:Class,
        owl:Class,
        dpv-owl:RiskConcept,
        risk-owl:PotentialConsequence,
        risk-owl:PotentialImpact,
        risk-owl:PotentialRisk ;
    dct:contributor _:N0a43dd9ea5e94fe695d8b7df8802cfdd ;
    dct:created "2024-02-14"^^xsd:date ;
    dct:source "DGA 28.3"@en ;
    rdfs:isDefinedBy eu-dga-owl: ;
    rdfs:subClassOf eu-dga-owl:A28-Impact,
        eu-dga-owl:DGARightsImpact ;
    sw:term_status "accepted"@en ;
    skos:definition "Something that acts as or is considered as an impact on Right of natural and legal persons to get a review by an impartial body with the appropriate expertise"@en ;
    skos:prefLabel "Impact on A28-3 Right to Impartial Review"@en .

eu-dga-owl:A28-Impact a rdfs:Class,
        owl:Class,
        dpv-owl:RiskConcept,
        risk-owl:PotentialConsequence,
        risk-owl:PotentialImpact,
        risk-owl:PotentialRisk ;
    dct:contributor _:N0a43dd9ea5e94fe695d8b7df8802cfdd ;
    dct:created "2024-12-17"^^xsd:date ;
    dct:source "DGA 28"@en ;
    rdfs:isDefinedBy eu-dga-owl: ;
    rdfs:subClassOf eu-dga-owl:DGARightsImpact ;
    sw:term_status "accepted"@en ;
    skos:definition "Something that acts as or is considered as an impact on Right of affected natural and legal persons to an effective judicial remedy"@en ;
    skos:prefLabel "Impact on A28 Right to an effective judicial remedy"@en .

eu-dga-owl:A31-2-Transfer-Agreement a rdfs:Class,
        owl:Class,
        dpv-owl:LegalBasis ;
    dct:contributor _:N458008bc6195484e9cc557f70eabda31 ;
    dct:created "2024-02-14"^^xsd:date ;
    dct:source [ a schema:WebPage ;
            schema:name "DGA 31.2" ;
            schema:url "https://eur-lex.europa.eu/eli/reg/2022/868/art_31/par_2/oj" ] ;
    rdfs:isDefinedBy eu-dga-owl: ;
    rdfs:subClassOf dpv-owl:DataTransferLegalBasis ;
    sw:term_status "accepted"@en ;
    skos:definition "Data Transfer International Agreement"@en ;
    skos:prefLabel "Art 31(2) Data Transfer International Agreement"@en .

eu-dga-owl:A31-3-Third-Country-Judgement a rdfs:Class,
        owl:Class,
        dpv-owl:LegalBasis ;
    dct:contributor _:N458008bc6195484e9cc557f70eabda31 ;
    dct:created "2024-02-14"^^xsd:date ;
    dct:source [ a schema:WebPage ;
            schema:name "DGA 31.3" ;
            schema:url "https://eur-lex.europa.eu/eli/reg/2022/868/art_31/par_3/oj" ] ;
    rdfs:isDefinedBy eu-dga-owl: ;
    rdfs:subClassOf dpv-owl:DataTransferLegalBasis ;
    sw:term_status "accepted"@en ;
    skos:definition "Data Transfer Third Country Judgement"@en ;
    skos:prefLabel "Art 31(3) Data Transfer Third Country Judgement"@en .

eu-dga-owl:A5-11-MCC a rdfs:Class,
        owl:Class,
        dpv-owl:LegalBasis ;
    dct:contributor _:N458008bc6195484e9cc557f70eabda31 ;
    dct:created "2024-02-14"^^xsd:date ;
    dct:source [ a schema:WebPage ;
            schema:name "DGA 5.11" ;
            schema:url "https://eur-lex.europa.eu/eli/reg/2022/868/art_5/par_11/oj" ] ;
    rdfs:isDefinedBy eu-dga-owl: ;
    rdfs:subClassOf dpv-owl:DataTransferLegalBasis ;
    sw:term_status "accepted"@en ;
    skos:definition "Model Contractual Clauses"@en ;
    skos:prefLabel "Art 5(11) Model Contractual Clauses"@en .

eu-dga-owl:A5-12-Adequacy-Decision a rdfs:Class,
        owl:Class,
        dpv-owl:LegalBasis ;
    dct:contributor _:N458008bc6195484e9cc557f70eabda31 ;
    dct:created "2024-02-14"^^xsd:date ;
    dct:source [ a schema:WebPage ;
            schema:name "DGA 5.12" ;
            schema:url "https://eur-lex.europa.eu/eli/reg/2022/868/art_5/par_12/oj" ] ;
    rdfs:isDefinedBy eu-dga-owl: ;
    rdfs:subClassOf dpv-owl:DataTransferLegalBasis ;
    sw:term_status "accepted"@en ;
    skos:definition "Adequacy Decision permitting the transfer of data"@en ;
    skos:prefLabel "Art 5(12) Adequacy Decision"@en .

eu-dga-owl:A5-9-Transfer-Permission a rdfs:Class,
        owl:Class,
        dpv-owl:LegalBasis ;
    dct:contributor _:N458008bc6195484e9cc557f70eabda31 ;
    dct:created "2024-02-14"^^xsd:date ;
    dct:source [ a schema:WebPage ;
            schema:name "DGA 5.9" ;
            schema:url "https://eur-lex.europa.eu/eli/reg/2022/868/art_5/par_9/oj" ] ;
    rdfs:isDefinedBy eu-dga-owl: ;
    rdfs:subClassOf dpv-owl:DataTransferLegalBasis ;
    sw:term_status "accepted"@en ;
    skos:definition "The legal basis justifying processing of non-personal data based on the permission of an entity to transfer data"@en ;
    skos:prefLabel "Art 5(9) Permission for Transfer"@en .

eu-dga-owl:A9-2 a rdfs:Class,
        owl:Class,
        dpv-owl:Right ;
    dct:contributor _:N0a43dd9ea5e94fe695d8b7df8802cfdd ;
    dct:created "2024-12-17"^^xsd:date ;
    dct:source "DGA 9-3"@en ;
    rdfs:isDefinedBy eu-dga-owl: ;
    rdfs:subClassOf dpv-owl:Right ;
    sw:term_status "accepted"@en ;
    skos:definition "Right of redress for a natural or legal person directly affected by a decision regarding reuse (A9-1), in the Member State where the relevant body is located"@en ;
    skos:prefLabel "A9-2 Right to Redress"@en .

eu-dga-owl:A9-2-Impact a rdfs:Class,
        owl:Class,
        dpv-owl:RiskConcept,
        risk-owl:PotentialConsequence,
        risk-owl:PotentialImpact,
        risk-owl:PotentialRisk ;
    dct:contributor _:N0a43dd9ea5e94fe695d8b7df8802cfdd ;
    dct:created "2024-12-17"^^xsd:date ;
    dct:source "DGA 9-3"@en ;
    rdfs:isDefinedBy eu-dga-owl: ;
    rdfs:subClassOf eu-dga-owl:DGARightsImpact ;
    sw:term_status "accepted"@en ;
    skos:definition "Something that acts as or is considered as an impact on Right of redress for a natural or legal person directly affected by a decision regarding reuse (A9-1), in the Member State where the relevant body is located"@en ;
    skos:prefLabel "Impact on A9-2 Right to Redress"@en .

eu-dga-owl:DAORegister a rdfs:Class,
        owl:Class,
        dpv-owl:PublicRegisterOfEntities ;
    dct:contributor _:N458008bc6195484e9cc557f70eabda31 ;
    dct:created "2024-02-14"^^xsd:date ;
    dct:source "DGA 19.5"@en ;
    rdfs:isDefinedBy eu-dga-owl: ;
    rdfs:subClassOf dpv-owl:PublicRegisterOfEntities ;
    sw:term_status "accepted"@en ;
    skos:definition "Registry containing list of recognised data altruism organisations"@en ;
    skos:prefLabel "Public Register of Data Altruism Organisations"@en .

eu-dga-owl:DAORegisterEU a rdfs:Class,
        owl:Class,
        dpv-owl:PublicRegisterOfEntities ;
    dct:contributor _:N458008bc6195484e9cc557f70eabda31 ;
    dct:created "2024-02-14"^^xsd:date ;
    dct:source "DGA 19.5"@en ;
    rdfs:isDefinedBy eu-dga-owl: ;
    rdfs:subClassOf dpv-owl:PublicRegisterOfEntities ;
    sw:term_status "accepted"@en ;
    skos:definition "Registry maintained by EU containing list of recognised data altruism organisations"@en ;
    skos:prefLabel "EU's Public Register of Data Altruism Organisations"@en .

eu-dga-owl:DAORegisterNational a rdfs:Class,
        owl:Class,
        dpv-owl:PublicRegisterOfEntities ;
    dct:contributor _:N458008bc6195484e9cc557f70eabda31 ;
    dct:created "2024-02-14"^^xsd:date ;
    dct:source "DGA 19.6"@en ;
    rdfs:isDefinedBy eu-dga-owl: ;
    rdfs:subClassOf dpv-owl:PublicRegisterOfEntities ;
    sw:term_status "accepted"@en ;
    skos:definition "Registry maintained at National level containing list of recognised data altruism organisations"@en ;
    skos:prefLabel "National Public Register of Data Altruism Organisations"@en .

eu-dga-owl:DGAComplianceUnknown a rdfs:Class,
        owl:Class,
        dpv-owl:Lawfulness ;
    dct:contributor _:N0a43dd9ea5e94fe695d8b7df8802cfdd,
        _:N458008bc6195484e9cc557f70eabda31 ;
    dct:created "2024-07-21"^^xsd:date ;
    rdfs:isDefinedBy eu-dga-owl: ;
    rdfs:subClassOf eu-dga-owl:DGALawfulness ;
    sw:term_status "accepted"@en ;
    skos:definition "State where lawfulness or compliance with DGA is unknown"@en ;
    skos:prefLabel "DGA Compliance Unknown"@en .

eu-dga-owl:DGACompliant a rdfs:Class,
        owl:Class,
        dpv-owl:Lawfulness ;
    dct:contributor _:N0a43dd9ea5e94fe695d8b7df8802cfdd,
        _:N458008bc6195484e9cc557f70eabda31 ;
    dct:created "2024-07-21"^^xsd:date ;
    rdfs:isDefinedBy eu-dga-owl: ;
    rdfs:subClassOf eu-dga-owl:DGALawfulness ;
    sw:term_status "accepted"@en ;
    skos:definition "State of being lawful or legally compliant for DGA"@en ;
    skos:prefLabel "DGA Compliant"@en .

eu-dga-owl:DGALawfulness a rdfs:Class,
        owl:Class,
        dpv-owl:Lawfulness ;
    dct:contributor _:N0a43dd9ea5e94fe695d8b7df8802cfdd,
        _:N458008bc6195484e9cc557f70eabda31 ;
    dct:created "2024-07-21"^^xsd:date ;
    rdfs:isDefinedBy eu-dga-owl: ;
    rdfs:subClassOf dpv-owl:Lawfulness ;
    sw:term_status "accepted"@en ;
    skos:definition "Status or state associated with being lawful or legally compliant regarding DGA"@en ;
    skos:prefLabel "DGA Lawfulness"@en .

eu-dga-owl:DGANonCompliant a rdfs:Class,
        owl:Class,
        dpv-owl:Lawfulness ;
    dct:contributor _:N0a43dd9ea5e94fe695d8b7df8802cfdd,
        _:N458008bc6195484e9cc557f70eabda31 ;
    dct:created "2024-07-21"^^xsd:date ;
    rdfs:isDefinedBy eu-dga-owl: ;
    rdfs:subClassOf eu-dga-owl:DGALawfulness ;
    sw:term_status "accepted"@en ;
    skos:definition "State of being unlawful or legally non-compliant for DGA"@en ;
    skos:prefLabel "DGA Non-compliant"@en .

eu-dga-owl:DGARightsImpact a rdfs:Class,
        owl:Class,
        dpv-owl:RiskConcept,
        risk-owl:PotentialConsequence,
        risk-owl:PotentialImpact,
        risk-owl:PotentialRisk ;
    dct:created "2024-12-01"^^xsd:date ;
    rdfs:isDefinedBy eu-dga-owl: ;
    rdfs:subClassOf risk-owl:RightsImpact ;
    sw:term_status "accepted"@en ;
    skos:definition "Something that acts as or is considered as an impact on one or more rights defined by DGA"@en ;
    skos:prefLabel "DGA Rights Impact"@en .

eu-dga-owl:DISP a rdfs:Class,
        owl:Class ;
    dct:contributor _:N458008bc6195484e9cc557f70eabda31 ;
    dct:created "2024-02-14"^^xsd:date ;
    dct:source "DGA 2.11"@en ;
    rdfs:isDefinedBy eu-dga-owl: ;
    rdfs:subClassOf dpv-owl:LegalEntity ;
    sw:term_status "accepted"@en ;
    skos:definition "An entity who establishes commercial relationships for the data sharing between data subjects and data holders on the one hand and data users on the other"@en ;
    skos:prefLabel "Data Intermediation Service Provider"@en .

eu-dga-owl:DISPEUApproval a rdfs:Class,
        owl:Class,
        dpv-owl:OrganisationalMeasure ;
    dct:contributor _:N458008bc6195484e9cc557f70eabda31 ;
    dct:created "2024-02-14"^^xsd:date ;
    dct:source "DGA 11.9"@en ;
    rdfs:isDefinedBy eu-dga-owl: ;
    rdfs:subClassOf dpv-owl:CertificationSeal ;
    sw:term_status "accepted"@en ;
    skos:definition "Confirmation and approval by a competent authority for the Data Intermediation Service Provider's compliance with Article 11 and Article 12 of the DGA"@en ;
    skos:prefLabel "EU Approval for Data Intermediation Service Provider"@en .

eu-dga-owl:DISPForDataHolder a rdfs:Class,
        owl:Class ;
    dct:contributor _:N458008bc6195484e9cc557f70eabda31 ;
    dct:created "2024-02-14"^^xsd:date ;
    dct:source "DGA 10.a"@en ;
    rdfs:isDefinedBy eu-dga-owl: ;
    rdfs:subClassOf eu-dga-owl:DISP ;
    sw:term_status "accepted"@en ;
    skos:definition "An entity who makes data holders' data available for potential data users, including bilateral or multilateral exchanges of data and platforms and databases for the joint exploitation of data"@en ;
    skos:prefLabel "Data Intermediation Service Provider for Data Holder"@en .

eu-dga-owl:DISPForDataSubject a rdfs:Class,
        owl:Class ;
    dct:contributor _:N458008bc6195484e9cc557f70eabda31 ;
    dct:created "2024-02-14"^^xsd:date ;
    dct:source "DGA 10.b"@en ;
    rdfs:isDefinedBy eu-dga-owl: ;
    rdfs:subClassOf eu-dga-owl:DISP ;
    sw:term_status "accepted"@en ;
    skos:definition "An entity who makes data subjects' personal data available for potential data users"@en ;
    skos:prefLabel "Data Intermediation Service Provider for Data Subject"@en .

eu-dga-owl:DISPNotice a rdfs:Class,
        owl:Class,
        dpv-owl:OrganisationalMeasure ;
    dct:contributor _:N458008bc6195484e9cc557f70eabda31 ;
    dct:created "2024-02-14"^^xsd:date ;
    dct:source " DGA 11.12"@en,
        " DGA 11.13"@en,
        " DGA 11.9"@en,
        "DGA 11.1"@en ;
    rdfs:isDefinedBy eu-dga-owl: ;
    rdfs:subClassOf dpv-owl:Notice ;
    sw:term_status "accepted"@en ;
    skos:definition "Notification by a Data Intermediation Service Provider to a competent authority concerning changes to details regarding its Data Intermediation Service"@en ;
    skos:prefLabel "Data Intermediation Service Notification"@en .

eu-dga-owl:DISPRegister a rdfs:Class,
        owl:Class,
        dpv-owl:PublicRegisterOfEntities ;
    dct:contributor _:N458008bc6195484e9cc557f70eabda31 ;
    dct:created "2024-02-14"^^xsd:date ;
    dct:source "DGA 11.10"@en ;
    rdfs:isDefinedBy eu-dga-owl: ;
    rdfs:subClassOf dpv-owl:PublicRegisterOfEntities ;
    sw:term_status "accepted"@en ;
    skos:definition "Document that contains a publicly available list of data intermediation service providers"@en ;
    skos:prefLabel "Public Register of Data Intermediation Service Providers"@en .

eu-dga-owl:DataAltruismAnnualReport a rdfs:Class,
        owl:Class,
        dpv-owl:OrganisationalMeasure ;
    dct:contributor _:N458008bc6195484e9cc557f70eabda31 ;
    dct:created "2024-02-14"^^xsd:date ;
    dct:source "DGA 20.2"@en ;
    rdfs:isDefinedBy eu-dga-owl: ;
    rdfs:subClassOf dpv-owl:RecordsOfActivities ;
    sw:term_status "accepted"@en ;
    skos:definition "Document containing the annual activities reported by a Data Altruism organisation"@en ;
    skos:prefLabel "Data Altruism Annual Activity Report"@en .

eu-dga-owl:DataAltruismAuthority a rdfs:Class,
        owl:Class ;
    dct:contributor _:N458008bc6195484e9cc557f70eabda31 ;
    dct:created "2024-02-14"^^xsd:date ;
    dct:source "DGA 23"@en ;
    rdfs:isDefinedBy eu-dga-owl: ;
    rdfs:subClassOf dpv-owl:Authority ;
    sw:term_status "accepted"@en ;
    skos:definition "An authority tasked with overseeing the activity of data altruism organisations and maintaining a public register of said entities"@en ;
    skos:prefLabel "Data Altruism Authority"@en .

eu-dga-owl:DataAltruismNotice a rdfs:Class,
        owl:Class,
        dpv-owl:OrganisationalMeasure ;
    dct:contributor _:N458008bc6195484e9cc557f70eabda31 ;
    dct:created "2024-02-14"^^xsd:date ;
    dct:source "DGA 21.1"@en ;
    rdfs:isDefinedBy eu-dga-owl: ;
    rdfs:subClassOf dpv-owl:Notice ;
    sw:term_status "accepted"@en ;
    skos:definition "Notice providing information regarding the processing of data for data altruistic purposes"@en ;
    skos:prefLabel "Data Altruism Notice"@en .

eu-dga-owl:DataAltruismOrganisation a rdfs:Class,
        owl:Class ;
    dct:contributor _:N458008bc6195484e9cc557f70eabda31 ;
    dct:created "2024-02-14"^^xsd:date ;
    dct:source " 18"@en,
        "DGA 2.16"@en ;
    rdfs:isDefinedBy eu-dga-owl: ;
    rdfs:subClassOf dpv-owl:NonProfitOrganisation ;
    sw:term_status "accepted"@en ;
    skos:definition "An non-profit organisation who collects and shares data for altruistic purposes"@en ;
    skos:prefLabel "Data Altruism Organisation"@en .

eu-dga-owl:DataAltruismRecord a rdfs:Class,
        owl:Class,
        dpv-owl:OrganisationalMeasure ;
    dct:contributor _:N458008bc6195484e9cc557f70eabda31 ;
    dct:created "2024-02-14"^^xsd:date ;
    dct:source "DGA 20"@en ;
    rdfs:isDefinedBy eu-dga-owl: ;
    rdfs:subClassOf dpv-owl:RecordsOfActivities ;
    sw:term_status "accepted"@en ;
    skos:definition "Document that logs the activity of the data altruism organisation"@en ;
    skos:prefLabel "Record of Data Altruism Activity"@en .

eu-dga-owl:DataAssetList a rdfs:Class,
        owl:Class,
        dpv-owl:OrganisationalMeasure ;
    dct:contributor _:N458008bc6195484e9cc557f70eabda31 ;
    dct:created "2024-02-14"^^xsd:date ;
    dct:source "DGA 8.2"@en ;
    rdfs:isDefinedBy eu-dga-owl: ;
    rdfs:subClassOf dpv-owl:OrganisationalMeasure ;
    sw:term_status "accepted"@en ;
    skos:definition "Searchable asset list which contains available data resources including their data format and size and the conditions for their re-use"@en ;
    skos:prefLabel "Data Asset List"@en .

eu-dga-owl:DataCooperative a rdfs:Class,
        owl:Class ;
    dct:contributor _:N458008bc6195484e9cc557f70eabda31 ;
    dct:created "2024-02-14"^^xsd:date ;
    dct:source " 10.c"@en,
        "DGA 2.15"@en ;
    rdfs:isDefinedBy eu-dga-owl: ;
    rdfs:subClassOf eu-dga-owl:DISP ;
    sw:term_status "accepted"@en ;
    skos:definition "An entity constituted by data subjects, one-person undertakings or SMEs who provides data intermediation services and supports its members in the exercise of their data-related rights"@en ;
    skos:prefLabel "Data Cooperative"@en .

eu-dga-owl:DataCooperativeService a rdfs:Class,
        owl:Class ;
    dct:contributor _:N458008bc6195484e9cc557f70eabda31 ;
    dct:created "2024-02-14"^^xsd:date ;
    rdfs:isDefinedBy eu-dga-owl: ;
    rdfs:subClassOf eu-dga-owl:DataIntermediationService ;
    sw:term_status "accepted"@en ;
    skos:definition "Service provided by a data cooperative"@en ;
    skos:prefLabel "Data Cooperative Service"@en .

eu-dga-owl:DataHolder a rdfs:Class,
        owl:Class ;
    dct:contributor _:N458008bc6195484e9cc557f70eabda31 ;
    dct:created "2024-02-14"^^xsd:date ;
    dct:source "DGA 2.8"@en ;
    rdfs:isDefinedBy eu-dga-owl: ;
    rdfs:subClassOf dpv-owl:LegalEntity ;
    sw:term_status "accepted"@en ;
    skos:definition "An entity who has the right to grant access to or to share certain personal data or non-personal data"@en ;
    skos:prefLabel "Data Holder"@en .

eu-dga-owl:DataIntermediationAuthority a rdfs:Class,
        owl:Class ;
    dct:contributor _:N458008bc6195484e9cc557f70eabda31 ;
    dct:created "2024-02-14"^^xsd:date ;
    dct:source "DGA 13"@en ;
    rdfs:isDefinedBy eu-dga-owl: ;
    rdfs:subClassOf dpv-owl:Authority ;
    sw:term_status "accepted"@en ;
    skos:definition "An authority tasked with overseeing the activity of data intermediation service providers and maintaining a public register of said entities"@en ;
    skos:prefLabel "Data Intermediation Authority"@en .

eu-dga-owl:DataIntermediationRecord a rdfs:Class,
        owl:Class,
        dpv-owl:OrganisationalMeasure ;
    dct:contributor _:N458008bc6195484e9cc557f70eabda31 ;
    dct:created "2024-02-14"^^xsd:date ;
    dct:source "DGA 12.o"@en ;
    rdfs:isDefinedBy eu-dga-owl: ;
    rdfs:subClassOf dpv-owl:RecordsOfActivities ;
    sw:term_status "accepted"@en ;
    skos:definition "Document that logs the activity of the data intermediation service provider"@en ;
    skos:prefLabel "Record of Data Intermediation Activity"@en .

eu-dga-owl:DataIntermediationService a rdfs:Class,
        owl:Class ;
    dct:contributor _:N458008bc6195484e9cc557f70eabda31 ;
    dct:created "2024-02-14"^^xsd:date ;
    dct:source "DGA 2.11"@en ;
    rdfs:isDefinedBy eu-dga-owl: ;
    rdfs:subClassOf dpv-owl:Service ;
    sw:term_status "accepted"@en ;
    skos:definition "Service of data intermediation which aims to facilitate the sharing of data between Data Subjects, Data Holders and Data Users"@en ;
    skos:prefLabel "Data Intermediation Service"@en .

eu-dga-owl:DataIntermediationServiceBetweenHoldersUsers a rdfs:Class,
        owl:Class ;
    dct:contributor _:N458008bc6195484e9cc557f70eabda31 ;
    dct:created "2024-02-14"^^xsd:date ;
    dct:source "DGA 10.a"@en ;
    rdfs:isDefinedBy eu-dga-owl: ;
    rdfs:subClassOf eu-dga-owl:DataIntermediationService ;
    sw:term_status "accepted"@en ;
    skos:definition "Data intermediation service for data shared between Data Holders and Data Users"@en ;
    skos:prefLabel "Data Intermediation Service between Data Holders and Data Users"@en .

eu-dga-owl:DataIntermediationServiceBetweenSubjectsUsers a rdfs:Class,
        owl:Class ;
    dct:contributor _:N458008bc6195484e9cc557f70eabda31 ;
    dct:created "2024-02-14"^^xsd:date ;
    dct:source "DGA 10.b"@en ;
    rdfs:isDefinedBy eu-dga-owl: ;
    rdfs:subClassOf eu-dga-owl:DataIntermediationService ;
    sw:term_status "accepted"@en ;
    skos:definition "Data intermediation service for data shared between Data Subjects, Natural Persons who are Data Holders and Data Users"@en ;
    skos:prefLabel "Data Intermediation Service between Data Subjects and Data Users"@en .

eu-dga-owl:DataReuseAssistant a rdfs:Class,
        owl:Class ;
    dct:contributor _:N458008bc6195484e9cc557f70eabda31 ;
    dct:created "2024-02-14"^^xsd:date ;
    dct:source "DGA 7"@en ;
    rdfs:isDefinedBy eu-dga-owl: ;
    rdfs:subClassOf dpv-owl:Entity ;
    sw:term_status "accepted"@en ;
    skos:definition "An entity designated by the Member State to provide technical support and guidance to public sector bodies regarding access and reuse of data and for requesting consent and permissions"@en ;
    skos:prefLabel "Data Reuse Assistant"@en .

eu-dga-owl:DataReuseRequest a rdfs:Class,
        owl:Class,
        dpv-owl:OrganisationalMeasure ;
    dct:contributor _:N458008bc6195484e9cc557f70eabda31 ;
    dct:created "2024-02-14"^^xsd:date ;
    dct:source "DGA 5.1"@en ;
    rdfs:isDefinedBy eu-dga-owl: ;
    rdfs:subClassOf dpv-owl:OrganisationalMeasure ;
    sw:term_status "accepted"@en ;
    skos:definition "Procedure to handle requests and provide data for reuse via single information point"@en ;
    skos:prefLabel "Data Reuse Request"@en .

eu-dga-owl:DataUser a rdfs:Class,
        owl:Class ;
    dct:contributor _:N458008bc6195484e9cc557f70eabda31 ;
    dct:created "2024-02-14"^^xsd:date ;
    dct:source "DGA 2.9"@en ;
    rdfs:isDefinedBy eu-dga-owl: ;
    rdfs:subClassOf dpv-owl:LegalEntity ;
    sw:term_status "accepted"@en ;
    skos:definition "An entity who has access and the right to use personal or non-personal data for commercial or non-commercial purposes"@en ;
    skos:prefLabel "Data User"@en .

eu-dga-owl:EUDataAltruismConsentForm a rdfs:Class,
        owl:Class,
        dpv-owl:OrganisationalMeasure ;
    dct:contributor _:N458008bc6195484e9cc557f70eabda31 ;
    dct:created "2024-02-14"^^xsd:date ;
    dct:source "DGA 25.1"@en ;
    rdfs:isDefinedBy eu-dga-owl: ;
    rdfs:subClassOf dpv-owl:ConsentManagement ;
    sw:term_status "accepted"@en ;
    skos:definition "A form provided by the European Commission for collecting consent"@en ;
    skos:prefLabel "European Data Altruism Consent Form"@en .

eu-dga-owl:EUSIPProvider a rdfs:Class,
        owl:Class ;
    dct:contributor _:N458008bc6195484e9cc557f70eabda31 ;
    dct:created "2024-02-14"^^xsd:date ;
    dct:source "DGA 8.4"@en ;
    rdfs:isDefinedBy eu-dga-owl: ;
    rdfs:subClassOf eu-dga-owl:SIPProvider ;
    sw:term_status "accepted"@en ;
    skos:definition "An entity who is responsible for receiving and transmitting requests for the reuse of public data in the EU"@en ;
    skos:prefLabel "EU Single Information Point Provider"@en .

eu-dga-owl:EuropeanDataInnovationBoard a rdfs:Class,
        owl:Class ;
    dct:contributor _:N458008bc6195484e9cc557f70eabda31 ;
    dct:created "2024-02-14"^^xsd:date ;
    dct:source "DGA 29"@en ;
    rdfs:isDefinedBy eu-dga-owl: ;
    rdfs:subClassOf dpv-owl:SupraNationalAuthority ;
    sw:term_status "accepted"@en ;
    skos:definition "An authority tasked with overseeing the activities of data intermediation service providers and data altruism organisations"@en ;
    skos:prefLabel "European Data Innovation Board"@en .

eu-dga-owl:LegalRepresentative a rdfs:Class,
        owl:Class ;
    dct:contributor _:N05cd1f43dbaf4b4ba297dab5ee221394 ;
    dct:created "2025-01-01"^^xsd:date ;
    dct:source "DGA 2.21"@en ;
    rdfs:isDefinedBy eu-dga-owl: ;
    rdfs:subClassOf dpv-owl:Representative ;
    sw:term_status "accepted"@en ;
    skos:definition "Legal Representative' means a natural or legal person established in the Union explicitly designated to act on behalf of a data intermediation services provider or an entity that collects data for objectives of general interest made available by natural or legal persons on the basis of data altruism not established in the Union, which may be addressed by the competent authorities for data intermediation services and the competent authorities for the registration of data altruism organisations in addition to or instead of the data intermediation services provider or entity with regard to the obligations under this Regulation, including with regard to initiating enforcement proceedings against a non-compliant data intermediation services provider or entity not established in the Union"@en ;
    skos:prefLabel "Legal Representative"@en .

eu-dga-owl:LocalSIPProvider a rdfs:Class,
        owl:Class ;
    dct:contributor _:N458008bc6195484e9cc557f70eabda31 ;
    dct:created "2024-02-14"^^xsd:date ;
    rdfs:isDefinedBy eu-dga-owl: ;
    rdfs:subClassOf eu-dga-owl:SIPProvider ;
    sw:term_status "accepted"@en ;
    skos:definition "A local entity who is responsible for receiving and transmitting requests for the reuse of public data"@en ;
    skos:prefLabel "Local Single Information Point Provider"@en .

eu-dga-owl:NationalDataAltruismPolicy a rdfs:Class,
        owl:Class,
        dpv-owl:OrganisationalMeasure ;
    dct:contributor _:N458008bc6195484e9cc557f70eabda31 ;
    dct:created "2024-02-14"^^xsd:date ;
    dct:source "DGA 16"@en ;
    rdfs:isDefinedBy eu-dga-owl: ;
    rdfs:subClassOf dpv-owl:Policy ;
    sw:term_status "accepted"@en ;
    skos:definition "A Policy established at National level regarding Data Altruism"@en ;
    skos:prefLabel "National Data Altruism Policy"@en .

eu-dga-owl:NationalSIPProvider a rdfs:Class,
        owl:Class ;
    dct:contributor _:N458008bc6195484e9cc557f70eabda31 ;
    dct:created "2024-02-14"^^xsd:date ;
    rdfs:isDefinedBy eu-dga-owl: ;
    rdfs:subClassOf eu-dga-owl:SIPProvider ;
    sw:term_status "accepted"@en ;
    skos:definition "A national entity who is responsible for receiving and transmitting requests for the reuse of public data"@en ;
    skos:prefLabel "National Single Information Point Provider"@en .

eu-dga-owl:PersonalDataReuseNotice a rdfs:Class,
        owl:Class,
        dpv-owl:OrganisationalMeasure ;
    dct:contributor _:N458008bc6195484e9cc557f70eabda31 ;
    dct:created "2024-02-14"^^xsd:date ;
    dct:source "DGA 12.m"@en ;
    rdfs:isDefinedBy eu-dga-owl: ;
    rdfs:subClassOf dpv-owl:ConsentNotice ;
    sw:term_status "accepted"@en ;
    skos:definition "Notice for data subjects to provide consent based on information and advise regarding intended use of data, exercise of rights, and applicable terms and conditions"@en ;
    skos:prefLabel "Personal Data Reuse Notice"@en .

eu-dga-owl:PublicLawGovernedBody a rdfs:Class,
        owl:Class ;
    dct:contributor _:N05cd1f43dbaf4b4ba297dab5ee221394 ;
    dct:created "2025-01-01"^^xsd:date ;
    dct:source "DGA 2.18"@en ;
    rdfs:isDefinedBy eu-dga-owl: ;
    rdfs:subClassOf dpv-owl:LegalEntity ;
    sw:term_status "accepted"@en ;
    skos:definition "Public Law Governed Body' or 'Body Governed by Public Law' means bodies that have the following characteristics: (a) they are established for the specific purpose of meeting needs in the general interest, and do not have an industrial or commercial character; (b) they have legal personality; (c) they are financed, for the most part, by the State, regional or local authorities, or other bodies governed by public law, are subject to management supervision by those authorities or bodies, or have an administrative, managerial or supervisory board, more than half of whose members are appointed by the State, regional or local authorities, or by other bodies governed by public law;"@en ;
    skos:prefLabel "Public Law Governed Body"@en .

eu-dga-owl:PublicSectorBody a rdfs:Class,
        owl:Class ;
    dct:contributor _:N05cd1f43dbaf4b4ba297dab5ee221394 ;
    dct:created "2025-01-01"^^xsd:date ;
    dct:source "DGA 2.17"@en ;
    rdfs:isDefinedBy eu-dga-owl: ;
    rdfs:subClassOf dpv-owl:PublicSectorBody ;
    sw:term_status "accepted"@en ;
    skos:definition "‘Public Sector Body’ means the State, regional or local authorities, bodies governed by public law or associations formed by one or more such authorities, or one or more such bodies governed by public law"@en ;
    skos:prefLabel "Public Sector Body"@en .

eu-dga-owl:RegionalSIPProvider a rdfs:Class,
        owl:Class ;
    dct:contributor _:N458008bc6195484e9cc557f70eabda31 ;
    dct:created "2024-02-14"^^xsd:date ;
    rdfs:isDefinedBy eu-dga-owl: ;
    rdfs:subClassOf eu-dga-owl:SIPProvider ;
    sw:term_status "accepted"@en ;
    skos:definition "A regional entity who is responsible for receiving and transmitting requests for the reuse of public data"@en ;
    skos:prefLabel "Regional Single Information Point Provider"@en .

eu-dga-owl:SIPProvider a rdfs:Class,
        owl:Class ;
    dct:contributor _:N458008bc6195484e9cc557f70eabda31 ;
    dct:created "2024-02-14"^^xsd:date ;
    dct:source "DGA 8"@en ;
    rdfs:isDefinedBy eu-dga-owl: ;
    rdfs:subClassOf dpv-owl:LegalEntity ;
    sw:term_status "accepted"@en ;
    skos:definition "An entity who is responsible for receiving and transmitting requests for the reuse of public data"@en ;
    skos:prefLabel "Single Information Point Provider"@en .

eu-dga-owl:SectorialSIPProvider a rdfs:Class,
        owl:Class ;
    dct:contributor _:N458008bc6195484e9cc557f70eabda31 ;
    dct:created "2024-02-14"^^xsd:date ;
    rdfs:isDefinedBy eu-dga-owl: ;
    rdfs:subClassOf eu-dga-owl:SIPProvider ;
    sw:term_status "accepted"@en ;
    skos:definition "An entity who is responsible for receiving and transmitting requests for the reuse of public data for a particular sector"@en ;
    skos:prefLabel "Sectorial Single Information Point Provider"@en .

eu-dga-owl:SecureProcessingEnvironment a rdfs:Class,
        owl:Class,
        dpv-owl:TechnicalMeasure ;
    dct:contributor _:N458008bc6195484e9cc557f70eabda31 ;
    dct:created "2024-02-14"^^xsd:date ;
    dct:source "DGA 2.20"@en ;
    rdfs:isDefinedBy eu-dga-owl: ;
    rdfs:subClassOf dpv-owl:SecureProcessingEnvironment ;
    sw:term_status "accepted"@en ;
    skos:definition "Physical or virtual environment to ensure compliance with EU law and allow the entity providing the secure processing environment to determine and supervise all data processing actions"@en ;
    skos:prefLabel "Secure Processing Environment"@en .

eu-dga-owl:SingleInformationPoint a rdfs:Class,
        owl:Class ;
    dct:contributor _:N458008bc6195484e9cc557f70eabda31 ;
    dct:created "2024-02-14"^^xsd:date ;
    rdfs:isDefinedBy eu-dga-owl: ;
    rdfs:subClassOf dpv-owl:Service ;
    sw:term_status "accepted"@en ;
    skos:definition "Service responsible for receiving and transmitting requests for the re-use of public data"@en ;
    skos:prefLabel "Single Information Point (SIP)"@en .

eu-dga-owl:ThirdCountryDataRequestNotice a rdfs:Class,
        owl:Class,
        dpv-owl:OrganisationalMeasure ;
    dct:contributor _:N458008bc6195484e9cc557f70eabda31 ;
    dct:created "2024-02-14"^^xsd:date ;
    dct:source "DGA 31.5"@en ;
    rdfs:isDefinedBy eu-dga-owl: ;
    rdfs:subClassOf dpv-owl:DataTransferNotice ;
    sw:term_status "accepted"@en ;
    skos:definition "Notice regarding a request of a third-country administrative authority to access data"@en ;
    skos:prefLabel "Third Country Data Request Notice"@en .

eu-dga-owl:hasDAO a rdf:Property,
        owl:ObjectProperty ;
    dcam:rangeIncludes eu-dga-owl:DataAltruismOrganisation ;
    dct:contributor _:N0a43dd9ea5e94fe695d8b7df8802cfdd,
        _:N458008bc6195484e9cc557f70eabda31 ;
    dct:created "2024-02-14"^^xsd:date ;
    rdfs:isDefinedBy eu-dga-owl: ;
    rdfs:subPropertyOf dpv-owl:hasEntity ;
    sw:term_status "accepted"@en ;
    skos:definition "Indicates association with data altruism organisation"@en ;
    skos:prefLabel "has data altruism organisation"@en ;
    schema:rangeIncludes eu-dga-owl:DataAltruismOrganisation .

eu-dga-owl:hasDISP a rdf:Property,
        owl:ObjectProperty ;
    dcam:rangeIncludes eu-dga-owl:DISP ;
    dct:contributor _:N0a43dd9ea5e94fe695d8b7df8802cfdd,
        _:N458008bc6195484e9cc557f70eabda31 ;
    dct:created "2024-02-14"^^xsd:date ;
    rdfs:isDefinedBy eu-dga-owl: ;
    rdfs:subPropertyOf dpv-owl:hasEntity ;
    sw:term_status "accepted"@en ;
    skos:definition "Indicates association with data intermediation service provider"@en ;
    skos:prefLabel "has data intermediation service provider"@en ;
    schema:rangeIncludes eu-dga-owl:DISP .

eu-dga-owl:hasDataHolder a rdf:Property,
        owl:ObjectProperty ;
    dcam:rangeIncludes eu-dga-owl:DataHolder ;
    dct:contributor _:N0a43dd9ea5e94fe695d8b7df8802cfdd,
        _:N458008bc6195484e9cc557f70eabda31 ;
    dct:created "2024-02-14"^^xsd:date ;
    rdfs:isDefinedBy eu-dga-owl: ;
    rdfs:subPropertyOf dpv-owl:hasEntity ;
    sw:term_status "accepted"@en ;
    skos:definition "Indicates association with data holder"@en ;
    skos:prefLabel "has data holder"@en ;
    schema:rangeIncludes eu-dga-owl:DataHolder .

eu-dga-owl:hasDataReuseAssistant a rdf:Property,
        owl:ObjectProperty ;
    dcam:rangeIncludes eu-dga-owl:DataReuseAssistant ;
    dct:contributor _:N0a43dd9ea5e94fe695d8b7df8802cfdd,
        _:N458008bc6195484e9cc557f70eabda31 ;
    dct:created "2024-02-14"^^xsd:date ;
    dct:source "DGA 7"@en ;
    rdfs:isDefinedBy eu-dga-owl: ;
    rdfs:subPropertyOf dpv-owl:hasEntity ;
    sw:term_status "accepted"@en ;
    skos:definition "Indicates association with competent body designated by the Member State to assist Public Bodies in activities related to data reuse"@en ;
    skos:prefLabel "has data reuse assistant"@en ;
    schema:rangeIncludes eu-dga-owl:DataReuseAssistant .

eu-dga-owl:hasDataUser a rdf:Property,
        owl:ObjectProperty ;
    dcam:rangeIncludes eu-dga-owl:DataUser ;
    dct:contributor _:N0a43dd9ea5e94fe695d8b7df8802cfdd,
        _:N458008bc6195484e9cc557f70eabda31 ;
    dct:created "2024-02-14"^^xsd:date ;
    rdfs:isDefinedBy eu-dga-owl: ;
    rdfs:subPropertyOf dpv-owl:hasEntity ;
    sw:term_status "accepted"@en ;
    skos:definition "Indicates association with data user"@en ;
    skos:prefLabel "has data user"@en ;
    schema:rangeIncludes eu-dga-owl:DataUser .

eu-dga-owl:serialisation-html a profile:ResourceDescriptor ;
    dct:conformsTo <https://www.w3.org/TR/html/> ;
    dct:format <https://www.iana.org/assignments/media-types/text/html> ;
    dct:title "EU Data Governance Act (DGA) - HTML serialiation" ;
    profile:hasArtifact <https://w3id.org/dpv/legal/eu/dga/eu-dga-owl.html> ;
    profile:hasRole role:specification .

eu-dga-owl:serialisation-jsonld a profile:ResourceDescriptor ;
    dct:conformsTo <https://www.w3.org/TR/json-ld11/> ;
    dct:format <https://www.iana.org/assignments/media-types/application/ld+json> ;
    dct:title "EU Data Governance Act (DGA) - JSON-LD serialiation" ;
    profile:hasArtifact <https://w3id.org/dpv/legal/eu/dga/eu-dga-owl.jsonld> ;
    profile:hasRole role:vocabulary .

eu-dga-owl:serialisation-n3 a profile:ResourceDescriptor ;
    dct:conformsTo <https://www.w3.org/TeamSubmission/n3/> ;
    dct:format <https://www.iana.org/assignments/media-types/text/n3> ;
    dct:title "EU Data Governance Act (DGA) - N3 serialiation" ;
    profile:hasArtifact <https://w3id.org/dpv/legal/eu/dga/eu-dga-owl.n3> ;
    profile:hasRole role:vocabulary .

eu-dga-owl:serialisation-rdf a profile:ResourceDescriptor ;
    dct:conformsTo rdf: ;
    dct:format <https://www.iana.org/assignments/media-types/application/rdf+xml> ;
    dct:title "EU Data Governance Act (DGA) - RDF/XML serialiation" ;
    profile:hasArtifact <https://w3id.org/dpv/legal/eu/dga/eu-dga-owl.rdf> ;
    profile:hasRole role:vocabulary .

eu-dga-owl:serialisation-ttl a profile:ResourceDescriptor ;
    dct:conformsTo <https://www.w3.org/TR/turtle/> ;
    dct:format <https://www.iana.org/assignments/media-types/text/turtle> ;
    dct:title "EU Data Governance Act (DGA) - Turtle serialiation" ;
    profile:hasArtifact <https://w3id.org/dpv/legal/eu/dga/eu-dga-owl.ttl> ;
    profile:hasRole role:vocabulary .

<https://w3id.org/dpv/examples> a profile:ResourceDescriptor ;
    dct:conformsTo <https://www.w3.org/TR/html/> ;
    dct:format <https://www.iana.org/assignments/media-types/text/html> ;
    dct:title "Examples for Data Privacy Vocabulary" ;
    profile:hasArtifact <https://w3id.org/dpv/examples> ;
    profile:hasRole role:guidance .

<https://w3id.org/dpv/guides> a profile:ResourceDescriptor ;
    dct:conformsTo <https://www.w3.org/TR/html/> ;
    dct:format <https://www.iana.org/assignments/media-types/text/html> ;
    dct:title "Guides for Data Privacy Vocabulary" ;
    profile:hasArtifact <https://w3id.org/dpv/guides> ;
    profile:hasRole role:guidance .

<https://w3id.org/dpv/primer> a profile:ResourceDescriptor ;
    dct:conformsTo <https://www.w3.org/TR/html/> ;
    dct:format <https://www.iana.org/assignments/media-types/text/html> ;
    dct:title "Primer for Data Privacy Vocabulary" ;
    profile:hasArtifact <https://w3id.org/dpv/primer> ;
    profile:hasRole role:guidance .

eu-dga-owl: a owl:Ontology,
        profile:Profile ;
    dct:bibliographicCitation "Harshvardhan J. Pandit, Beatriz Esteves, Georg P. Krog, Paul Ryan, Delaram Golpayegani, Julian Flake (2025) Data Privacy Vocabulary (DPV) – Version 2.0. In: Demartini, G., et al. The Semantic Web – ISWC 2024. ISWC 2024. Lecture Notes in Computer Science, vol 15233. Springer, Cham. https://doi.org/10.1007/978-3-031-77847-6_10" ;
    dct:conformsTo <http://www.w3.org/2002/07/owl>,
        "http://www.w3.org/2000/01/rdf-schema",
        "http://www.w3.org/2004/02/skos/core" ;
    dct:contributor _:N05cd1f43dbaf4b4ba297dab5ee221394,
        _:N0a43dd9ea5e94fe695d8b7df8802cfdd,
        _:N458008bc6195484e9cc557f70eabda31 ;
    dct:created "2023-09-20"@en ;
    dct:creator _:N05cd1f43dbaf4b4ba297dab5ee221394,
        _:N0a43dd9ea5e94fe695d8b7df8802cfdd,
        _:N458008bc6195484e9cc557f70eabda31 ;
    dct:description "Extension to the Data Privacy Vocabulary (DPV) providing concepts for representing  information associated with EU DGA"@en ;
    dct:hasVersion eu-dga-owl: ;
    dct:identifier "https://w3id.org/dpv/legal/eu/dga" ;
    dct:issued "2023-09-20"@en ;
    dct:license <https://www.w3.org/copyright/document-license-2023/> ;
    dct:modified "2025-03-16"@en ;
    dct:publisher <https://www.w3.org/> ;
    dct:source <https://www.w3.org/groups/cg/dpvcg/> ;
    dct:title "EU Data Governance Act (DGA)"@en ;
    bibo:doi "10.5281/zenodo.12505841" ;
    bibo:status "http://purl.org/ontology/bibo/status/published" ;
    vann:preferredNamespacePrefix "eu-dga" ;
    vann:preferredNamespaceUri "https://w3id.org/dpv/legal/eu/dga#" ;
    rdfs:Label "EU-DGA"@en ;
    owl:versionIRI <https://w3id.org/dpv/2.1/legal/eu/dga/owl#> ;
    owl:versionInfo "2.1" ;
    profile:hasResource <https://w3id.org/dpv/examples>,
        <https://w3id.org/dpv/guides>,
        eu-dga-owl:serialisation-html,
        eu-dga-owl:serialisation-jsonld,
        eu-dga-owl:serialisation-n3,
        eu-dga-owl:serialisation-rdf,
        eu-dga-owl:serialisation-ttl,
        <https://w3id.org/dpv/primer> ;
    profile:isProfileOf <http://www.w3.org/2002/07/owl>,
        eu-dga-owl:,
        <https://w3id.org/dpv/owl> ;
    foaf:logo <https://w3id.org/dpv/media/logo.png> ;
    schema:version "2.1" .

_:N2bfb2dfcc0b24c5182bd06c242c085fa a foaf:Organization ;
    foaf:name "Signatu AS" .

_:N313d89a6c37147bfac1bbb4aa7f6510b a foaf:Organization ;
    foaf:name "ADAPT Centre, Dublin City University" .

_:N3f64d3533a104953b63bb217ff4665c5 a foaf:Organization ;
    foaf:name "IDLab, IMEC, Ghent University" .

_:N05cd1f43dbaf4b4ba297dab5ee221394 a dct:Agent,
        foaf:Person ;
    org:memberOf _:N2bfb2dfcc0b24c5182bd06c242c085fa ;
    foaf:homepage "https://www.linkedin.com/in/georg-philip-krog-a2a278104/" ;
    foaf:name "Georg P. Krog" .

_:N0a43dd9ea5e94fe695d8b7df8802cfdd a dct:Agent,
        foaf:Person ;
    scoro:hasORCID "0000-0002-5068-3714" ;
    org:memberOf _:N313d89a6c37147bfac1bbb4aa7f6510b ;
    foaf:homepage "https://harshp.com/" ;
    foaf:name "Harshvardhan J. Pandit" .

_:N458008bc6195484e9cc557f70eabda31 a dct:Agent,
        foaf:Person ;
    scoro:hasORCID "0000-0003-0259-7560" ;
    org:memberOf _:N3f64d3533a104953b63bb217ff4665c5 ;
    foaf:name "Beatriz Esteves" .

