@prefix ai: <https://w3id.org/dpv/ai#> .
@prefix bibo: <http://purl.org/ontology/bibo/> .
@prefix dcam: <http://purl.org/dc/dcam/> .
@prefix dct: <http://purl.org/dc/terms/> .
@prefix dpv: <https://w3id.org/dpv#> .
@prefix eu-aiact: <https://w3id.org/dpv/legal/eu/aiact#> .
@prefix foaf: <http://xmlns.com/foaf/0.1/> .
@prefix org: <http://www.w3.org/ns/org#> .
@prefix owl: <http://www.w3.org/2002/07/owl#> .
@prefix pd: <https://w3id.org/dpv/pd#> .
@prefix profile: <http://www.w3.org/ns/dx/prof/> .
@prefix rdf: <http://www.w3.org/1999/02/22-rdf-syntax-ns#> .
@prefix rdfs: <http://www.w3.org/2000/01/rdf-schema#> .
@prefix risk: <https://w3id.org/dpv/risk#> .
@prefix role: <http://www.w3.org/ns/dx/prof/role/> .
@prefix schema: <https://schema.org/> .
@prefix scoro: <http://purl.org/spar/scoro/> .
@prefix skos: <http://www.w3.org/2004/02/skos/core#> .
@prefix sw: <http://www.w3.org/2003/06/sw-vocab-status/ns#> .
@prefix tech: <https://w3id.org/dpv/tech#> .
@prefix vann: <http://purl.org/vocab/vann/> .
@prefix xsd: <http://www.w3.org/2001/XMLSchema#> .

eu-aiact:AIActComplianceUnknown a rdfs:Class,
        skos:Concept,
        dpv:Lawfulness ;
    dct:contributor _:person-beatriz-esteves,
        _:person-harshvardhan-j-pandit ;
    dct:created "2024-07-21"^^xsd:date ;
    rdfs:isDefinedBy eu-aiact: ;
    sw:term_status "accepted"@en ;
    skos:broader eu-aiact:AIActLawfulness ;
    skos:definition "State where lawfulness or compliance with AI Act is unknown"@en ;
    skos:inScheme eu-aiact:compliance-classes ;
    skos:prefLabel "AI Act Compliance Unknown"@en .

eu-aiact:AIActCompliant a rdfs:Class,
        skos:Concept,
        dpv:Lawfulness ;
    dct:contributor _:person-beatriz-esteves,
        _:person-harshvardhan-j-pandit ;
    dct:created "2024-07-21"^^xsd:date ;
    rdfs:isDefinedBy eu-aiact: ;
    sw:term_status "accepted"@en ;
    skos:broader eu-aiact:AIActLawfulness ;
    skos:definition "State of being lawful or legally compliant for AI Act"@en ;
    skos:inScheme eu-aiact:compliance-classes ;
    skos:prefLabel "AI Act Compliant"@en .

eu-aiact:AIActLawfulness a rdfs:Class,
        skos:Concept,
        dpv:Lawfulness ;
    dct:contributor _:person-beatriz-esteves,
        _:person-harshvardhan-j-pandit ;
    dct:created "2024-07-21"^^xsd:date ;
    rdfs:isDefinedBy eu-aiact: ;
    sw:term_status "accepted"@en ;
    skos:broader dpv:Lawfulness ;
    skos:definition "Status or state associated with being lawful or legally compliant regarding AI Act"@en ;
    skos:inScheme eu-aiact:compliance-classes ;
    skos:prefLabel "AI Act Lawfulness"@en .

eu-aiact:AIActNonCompliant a rdfs:Class,
        skos:Concept,
        dpv:Lawfulness ;
    dct:contributor _:person-beatriz-esteves,
        _:person-harshvardhan-j-pandit ;
    dct:created "2024-07-21"^^xsd:date ;
    rdfs:isDefinedBy eu-aiact: ;
    sw:term_status "accepted"@en ;
    skos:broader eu-aiact:AIActLawfulness ;
    skos:definition "State of being unlawful or legally non-compliant for AI Act"@en ;
    skos:inScheme eu-aiact:compliance-classes ;
    skos:prefLabel "AI Act Non-compliant"@en .

eu-aiact:AIDeployer a rdfs:Class,
        skos:Concept ;
    dct:contributor _:person-delaram-golpayegani ;
    dct:created "2024-04-10"^^xsd:date ;
    dct:modified "2025-07-30"^^xsd:date ;
    dct:source "AIA (Art. 3(4))"@en ;
    rdfs:isDefinedBy eu-aiact: ;
    rdfs:subClassOf eu-aiact:AIOperator,
        tech:Deployer ;
    sw:term_status "modified"@en ;
    skos:broader eu-aiact:AIOperator,
        tech:Deployer ;
    skos:definition "A natural or legal person, public authority, agency or other body using an AI system under its authority except where the AI system is used in the course of a personal non-professional activity"@en ;
    skos:inScheme eu-aiact:roles-classes ;
    skos:prefLabel "AI Deployer"@en .

eu-aiact:AIDistributor a rdfs:Class,
        skos:Concept ;
    dct:contributor _:person-delaram-golpayegani ;
    dct:created "2024-04-10"^^xsd:date ;
    dct:source "AIA (Art. 3(7))"@en ;
    rdfs:isDefinedBy eu-aiact: ;
    rdfs:subClassOf eu-aiact:AIOperator,
        tech:Distributor ;
    sw:term_status "accepted"@en ;
    skos:broader eu-aiact:AIOperator,
        tech:Distributor ;
    skos:definition "A natural or legal person in the supply chain, other than the provider or the importer, that makes an AI system available on the Union market"@en ;
    skos:inScheme eu-aiact:roles-classes ;
    skos:prefLabel "AI Distributor"@en .

eu-aiact:AIImporter a rdfs:Class,
        skos:Concept ;
    dct:contributor _:person-delaram-golpayegani ;
    dct:created "2024-04-10"^^xsd:date ;
    dct:modified "2025-07-30"^^xsd:date ;
    dct:source "AIA (Art. 3(6))"@en ;
    rdfs:isDefinedBy eu-aiact: ;
    rdfs:subClassOf eu-aiact:AIOperator,
        tech:Importer ;
    sw:term_status "modified"@en ;
    skos:broader eu-aiact:AIOperator,
        tech:Importer ;
    skos:definition "A natural or legal person located or established in the Union that places on the market an AI system that bears the name or trademark of a natural or legal person established in a third country"@en ;
    skos:inScheme eu-aiact:roles-classes ;
    skos:prefLabel "AI Importer"@en .

eu-aiact:AILiteracy a rdfs:Class,
        skos:Concept,
        dpv:OrganisationalMeasure ;
    dct:contributor _:person-delaram-golpayegani ;
    dct:created "2024-04-10"^^xsd:date ;
    dct:modified "2026-02-09"^^xsd:date ;
    dct:source "AIA (Art. 3(56))"@en ;
    rdfs:isDefinedBy eu-aiact: ;
    sw:term_status "modified"@en ;
    skos:broader dpv:AILiteracy ;
    skos:definition "Skills, knowledge and understanding that allow providers, deployers and affected persons, taking into account their respective rights and obligations in the context of this Regulation, to make an informed deployment of AI systems, as well as to gain awareness about the opportunities and risks of AI and possible harm it can cause"@en ;
    skos:inScheme eu-aiact:misc-classes ;
    skos:prefLabel "AI Literacy"@en ;
    skos:scopeNote "AI Literacy should take into account the subject's level of technical knowledge, experience, education and training -- these can be represented through the corresponding concepts in the PD extension"@en .

eu-aiact:AIOffice a rdfs:Class,
        skos:Concept ;
    dct:contributor _:person-delaram-golpayegani ;
    dct:created "2024-04-10"^^xsd:date ;
    dct:modified "2027-07-30"^^xsd:date ;
    dct:source "AIA(Art. 3(47))"@en ;
    rdfs:isDefinedBy eu-aiact: ;
    rdfs:subClassOf dpv:Authority ;
    sw:term_status "modified"@en ;
    skos:broader dpv:Authority ;
    skos:definition "the Commission’s function of contributing to the implementation, monitoring and supervision of AI systems and general-purpose AI models, and AI governance, provided for in Commission Decision of 24 January 2024; references in the AI Act to the AI Office shall be construed as references to the Commission"@en ;
    skos:inScheme eu-aiact:roles-classes ;
    skos:prefLabel "Artificial Intelligence Office"@en .

eu-aiact:AIOperator a rdfs:Class,
        skos:Concept ;
    dct:contributor _:person-delaram-golpayegani ;
    dct:created "2024-04-10"^^xsd:date ;
    dct:modified "2025-07-30"^^xsd:date ;
    dct:source "AIA (Art. 3(8))"@en ;
    rdfs:isDefinedBy eu-aiact: ;
    rdfs:subClassOf tech:Operator ;
    sw:term_status "modified"@en ;
    skos:broader tech:Operator ;
    skos:definition "A provider, product manufacturer, deployer, authorised representative, importer or distributor"@en ;
    skos:inScheme eu-aiact:roles-classes ;
    skos:prefLabel "AI Operator"@en .

eu-aiact:AIProductManufacturer a rdfs:Class,
        skos:Concept ;
    dct:contributor _:person-delaram-golpayegani ;
    dct:created "2024-04-10"^^xsd:date ;
    dct:modified "2027-07-30"^^xsd:date ;
    rdfs:isDefinedBy eu-aiact: ;
    rdfs:subClassOf eu-aiact:AIOperator,
        tech:Manufacturer ;
    sw:term_status "modified"@en ;
    skos:broader eu-aiact:AIOperator,
        tech:Manufacturer ;
    skos:definition "Entity that manufactures an AI Product"@en ;
    skos:inScheme eu-aiact:roles-classes ;
    skos:prefLabel "AI Product Manufacturer"@en .

eu-aiact:AIProvider a rdfs:Class,
        skos:Concept ;
    dct:contributor _:person-delaram-golpayegani ;
    dct:created "2024-04-10"^^xsd:date ;
    dct:modified "2025-07-30"^^xsd:date ;
    dct:source "AIA (Art. 3(3))"@en ;
    rdfs:isDefinedBy eu-aiact: ;
    rdfs:subClassOf eu-aiact:AIOperator,
        tech:Provider ;
    sw:term_status "modified"@en ;
    skos:broader eu-aiact:AIOperator,
        tech:Provider ;
    skos:definition "A natural or legal person, public authority, agency or other body that develops an AI system or a general-purpose AI model or that has an AI system or a general-purpose AI model developed and places it on the market or puts the AI system into service under its own name or trademark, whether for payment or free of charge"@en ;
    skos:inScheme eu-aiact:roles-classes ;
    skos:prefLabel "AI Provider"@en .

eu-aiact:AIRegulatorySandbox a rdfs:Class,
        skos:Concept,
        dpv:OrganisationalMeasure ;
    dct:contributor _:person-delaram-golpayegani ;
    dct:created "2024-04-10"^^xsd:date ;
    dct:modified "2024-07-30"^^xsd:date ;
    dct:source "AIA (Art. 3(55))"@en ;
    rdfs:isDefinedBy eu-aiact: ;
    sw:term_status "modified"@en ;
    skos:broader dpv:RegulatorySandbox ;
    skos:definition "A controlled framework set up by a competent authority which offers providers or prospective providers of AI systems the possibility to develop, train, validate and test, where appropriate in real-world conditions, an innovative AI system, pursuant to a sandbox plan for a limited time under regulatory supervision"@en ;
    skos:inScheme eu-aiact:assessment-classes ;
    skos:prefLabel "AI Regulatory Sandbox"@en .

eu-aiact:AISystem a rdfs:Class,
        skos:Concept ;
    dct:contributor _:person-delaram-golpayegani ;
    dct:created "2024-04-10"^^xsd:date ;
    dct:source "AIA (Art. 3(1))"@en ;
    rdfs:isDefinedBy eu-aiact: ;
    rdfs:subClassOf ai:AISystem ;
    sw:term_status "accepted"@en ;
    skos:broader ai:AISystem ;
    skos:definition "A machine-based system designed to operate with varying levels of autonomy and that may exhibit adaptiveness after deployment and that, for explicit or implicit objectives, infers, from the input it receives, how to generate outputs such as predictions, content, recommendations, or decisions that can influence physical or virtual environments."@en ;
    skos:inScheme eu-aiact:system-classes ;
    skos:prefLabel "AI System"@en ;
    skos:scopeNote "Note All references to the AI Act referred to the provisional agreement published in Feb 2024"@en .

eu-aiact:AISystemPerformance a rdfs:Class,
        skos:Concept ;
    dct:contributor _:person-delaram-golpayegani ;
    dct:created "2024-04-10"^^xsd:date ;
    dct:source "AIA(Art. 3(18))"@en ;
    rdfs:isDefinedBy eu-aiact: ;
    sw:term_status "accepted"@en ;
    skos:definition "The ability of an AI system to achieve its intended purpose"@en ;
    skos:inScheme eu-aiact:assessment-classes ;
    skos:prefLabel "AI System Performance"@en .

eu-aiact:AsylumSector a rdfs:Class,
        skos:Concept,
        dpv:Sector ;
    dct:contributor _:person-delaram-golpayegani,
        _:person-harshvardhan-j-pandit ;
    dct:created "2024-12-01"^^xsd:date ;
    dct:source " Annex III"@en,
        "EU AI Act"@en ;
    rdfs:isDefinedBy eu-aiact: ;
    sw:term_status "accepted"@en ;
    skos:broader dpv:Sector ;
    skos:definition "Sector related to asylum management"@en ;
    skos:inScheme eu-aiact:sector-classes ;
    skos:prefLabel "Asylum Sector"@en .

eu-aiact:AuthorisedRepresentative a rdfs:Class,
        skos:Concept ;
    dct:contributor _:person-delaram-golpayegani ;
    dct:created "2024-04-10"^^xsd:date ;
    dct:source "AIA (Art. 3(5))"@en ;
    rdfs:isDefinedBy eu-aiact: ;
    rdfs:subClassOf dpv:Representative,
        eu-aiact:AIOperator ;
    sw:term_status "accepted"@en ;
    skos:broader dpv:Representative,
        eu-aiact:AIOperator ;
    skos:definition "A natural or legal person located or established in the Union who has received and accepted a written mandate from a provider of an AI system or a general-purpose AI model to, respectively, perform and carry out on its behalf the obligations and procedures established by the AI Act"@en ;
    skos:inScheme eu-aiact:roles-classes ;
    skos:prefLabel "Authorised Representative"@en .

eu-aiact:AvailableOnEUMarket a rdfs:Class,
        skos:Concept,
        eu-aiact:MarketAvailabilityStatus ;
    dct:contributor _:person-delaram-golpayegani ;
    dct:created "2024-05-17"^^xsd:date ;
    dct:source "AIA (Art. 3(10))"@en ;
    rdfs:isDefinedBy eu-aiact: ;
    sw:term_status "accepted"@en ;
    skos:broader eu-aiact:AvailableOnMarket ;
    skos:definition "Status associated with supply of an AI system or a general purpose AI model for distribution or use on the Union market in the course of a commercial activity, whether in return for payment or free of charge"@en ;
    skos:inScheme eu-aiact:status-classes ;
    skos:prefLabel "Available on EU Market"@en .

eu-aiact:AvailableOnMarket a rdfs:Class,
        skos:Concept,
        eu-aiact:MarketAvailabilityStatus ;
    dct:contributor _:person-delaram-golpayegani ;
    dct:created "2024-05-17"^^xsd:date ;
    dct:source "AIA (Art. 3(10))"@en ;
    rdfs:isDefinedBy eu-aiact: ;
    sw:term_status "accepted"@en ;
    skos:broader eu-aiact:MarketAvailabilityStatus ;
    skos:definition "Status associated with supply of an AI system or a general purpose AI model for distribution or use on the market in the course of a commercial activity, whether in return for payment or free of charge"@en ;
    skos:inScheme eu-aiact:status-classes ;
    skos:prefLabel "Available on Market"@en .

eu-aiact:AvailableOnNonEUMarket a rdfs:Class,
        skos:Concept,
        eu-aiact:MarketAvailabilityStatus ;
    dct:contributor _:person-delaram-golpayegani ;
    dct:created "2024-05-17"^^xsd:date ;
    rdfs:isDefinedBy eu-aiact: ;
    sw:term_status "accepted"@en ;
    skos:broader eu-aiact:AvailableOnMarket ;
    skos:definition "Status associated with supply of an AI system or a general purpose AI model for distribution or use on any market except the Union market in the course of a commercial activity, whether in return for payment or free of charge"@en ;
    skos:inScheme eu-aiact:status-classes ;
    skos:prefLabel "Available on Non-EU Market"@en .

eu-aiact:BiometricCategorisation a rdfs:Class,
        skos:Concept,
        tech:Capability ;
    dct:contributor _:person-delaram-golpayegani ;
    dct:created "2024-04-10"^^xsd:date ;
    dct:modified "2025-07-30"^^xsd:date ;
    dct:source "AIA Art. 3(40)"@en ;
    rdfs:isDefinedBy eu-aiact: ;
    sw:term_status "modified"@en ;
    skos:broader ai:BiometricCategorisation ;
    skos:definition "Capability where assigning natural persons to specific categories happens on the basis of their biometric data unless ancillary to another commercial service and strictly necessary for objective technical reasons"@en ;
    skos:inScheme eu-aiact:capability-classes ;
    skos:prefLabel "Biometric Categorisation"@en ;
    skos:related pd:Biometric .

eu-aiact:BiometricCategorisationSystem a rdfs:Class,
        skos:Concept,
        eu-aiact:AISystem ;
    dct:contributor _:person-delaram-golpayegani ;
    dct:created "2024-04-10"^^xsd:date ;
    dct:modified "2025-07-30"^^xsd:date ;
    dct:source "AIA(Art. 3(40))"@en ;
    rdfs:isDefinedBy eu-aiact: ;
    sw:term_status "modified"@en ;
    skos:broader eu-aiact:AISystem ;
    skos:definition "An AI system for the purpose of assigning natural persons to specific categories on the basis of their biometric data, unless it is ancillary to another commercial service and strictly necessary for objective technical reasons"@en ;
    skos:inScheme eu-aiact:system-classes ;
    skos:prefLabel "Biometric Categorisation System"@en ;
    skos:related pd:Biometric .

eu-aiact:BiometricData a rdfs:Class,
        skos:Concept,
        dpv:PersonalData ;
    dct:contributor _:person-delaram-golpayegani ;
    dct:created "2024-04-10"^^xsd:date ;
    dct:modified "2025-07-30"^^xsd:date ;
    dct:source "AIA(Art. 3(34))"@en ;
    rdfs:isDefinedBy eu-aiact: ;
    sw:term_status "accepted"@en ;
    skos:broader pd:Biometric ;
    skos:definition "Personal data resulting from specific technical processing relating to the physical, physiological or behavioural characteristics of a natural person, such as facial images or dactyloscopic data"@en ;
    skos:inScheme eu-aiact:data-classes ;
    skos:prefLabel "Biometric Data"@en .

eu-aiact:BiometricIdentification a rdfs:Class,
        skos:Concept,
        tech:Capability ;
    dct:contributor _:person-delaram-golpayegani ;
    dct:created "2024-04-10"^^xsd:date ;
    dct:modified "2025-07-30"^^xsd:date ;
    dct:source "AIA Art. 3(35)"@en ;
    rdfs:isDefinedBy eu-aiact: ;
    sw:term_status "modified"@en ;
    skos:broader ai:BiometricIdentification ;
    skos:definition "Capability where the automated recognition of physical, physiological, behavioural, and psychological human features are used for the purpose of establishing the identity of a natural person by comparing biometric data of that individual to to biometric data of individuals stored in a database"@en ;
    skos:inScheme eu-aiact:capability-classes ;
    skos:prefLabel "Biometric Identification"@en ;
    skos:related pd:Biometric .

eu-aiact:BiometricVerification a rdfs:Class,
        skos:Concept,
        tech:Capability ;
    dct:contributor _:person-delaram-golpayegani ;
    dct:created "2024-04-10"^^xsd:date ;
    dct:modified "2025-07-30"^^xsd:date ;
    dct:source "AIA Art.3 (36)"@en ;
    rdfs:isDefinedBy eu-aiact: ;
    sw:term_status "modified"@en ;
    skos:broader dpv:IdentityVerification ;
    skos:definition "The automated, one-to-one verification, including authentication, of the identity of natural persons by comparing their biometric data to previously provided biometric data"@en ;
    skos:inScheme eu-aiact:capability-classes ;
    skos:prefLabel "Biometric Verification"@en ;
    skos:related pd:Biometric .

eu-aiact:BorderControlSector a rdfs:Class,
        skos:Concept,
        dpv:Sector ;
    dct:contributor _:person-delaram-golpayegani,
        _:person-harshvardhan-j-pandit ;
    dct:created "2024-12-01"^^xsd:date ;
    dct:source " Annex III"@en,
        "EU AI Act"@en ;
    rdfs:isDefinedBy eu-aiact: ;
    sw:term_status "accepted"@en ;
    skos:broader dpv:Sector ;
    skos:definition "Sector related to border control management"@en ;
    skos:inScheme eu-aiact:sector-classes ;
    skos:prefLabel "Border Control Sector"@en .

eu-aiact:CEMarking a rdfs:Class,
        skos:Concept,
        dpv:OrganisationalMeasure ;
    dct:contributor _:person-delaram-golpayegani ;
    dct:created "2024-04-10"^^xsd:date ;
    dct:modified "2024-07-30"^^xsd:date ;
    dct:source "AIA(Art. 3(24))"@en ;
    rdfs:isDefinedBy eu-aiact: ;
    sw:term_status "modified"@en ;
    skos:broader dpv:CertificationSeal ;
    skos:definition "A marking by which a provider indicates that an AI system is in conformity with the requirements set out in Chapter III, Section 2 and other applicable Union harmonisation legislation providing for its affixing"@en ;
    skos:inScheme eu-aiact:assessment-classes ;
    skos:prefLabel "CE Marking"@en .

eu-aiact:ChangeCategory a rdfs:Class,
        skos:Concept ;
    dct:contributor _:person-delaram-golpayegani ;
    dct:created "2024-12-01"^^xsd:date ;
    rdfs:isDefinedBy eu-aiact: ;
    rdfs:subClassOf dpv:Context ;
    sw:term_status "accepted"@en ;
    skos:broader dpv:Context ;
    skos:definition "A categorisation of the change associated with the AI system"@en ;
    skos:inScheme eu-aiact:status-classes ;
    skos:prefLabel "Change Category"@en .

eu-aiact:ChangeDescription a rdfs:Class,
        skos:Concept ;
    dct:contributor _:person-delaram-golpayegani ;
    dct:created "2024-12-01"^^xsd:date ;
    rdfs:isDefinedBy eu-aiact: ;
    rdfs:subClassOf dpv:Context ;
    sw:term_status "accepted"@en ;
    skos:broader dpv:Context ;
    skos:definition "A description of the change associated with the AI system"@en ;
    skos:inScheme eu-aiact:status-classes ;
    skos:prefLabel "Change Description"@en .

eu-aiact:CommonSpecification a rdfs:Class,
        skos:Concept,
        tech:Documentation ;
    dct:contributor _:person-delaram-golpayegani ;
    dct:created "2024-04-10"^^xsd:date ;
    dct:modified "2024-12-17"^^xsd:date ;
    dct:source "AIA Art.3-28"@en ;
    rdfs:isDefinedBy eu-aiact: ;
    sw:term_status "modified"@en ;
    skos:broader tech:Specification ;
    skos:definition "A set of technical specifications, as defined in point 4 of Article 2 of Regulation (EU) No 1025/2012 providing means to comply with certain requirements established under the AI Act"@en ;
    skos:inScheme eu-aiact:docs-classes ;
    skos:prefLabel "Common Specification"@en .

eu-aiact:ConformityAssessment a rdfs:Class,
        skos:Concept,
        dpv:OrganisationalMeasure ;
    dct:contributor _:person-delaram-golpayegani ;
    dct:created "2024-04-10"^^xsd:date ;
    dct:modified "2024-07-30"^^xsd:date ;
    dct:source "AIA(Art. 3(20))"@en ;
    rdfs:isDefinedBy eu-aiact: ;
    sw:term_status "modified"@en ;
    skos:broader dpv:Assessment ;
    skos:definition "The process of demonstrating whether the requirements set out in Chapter III, Section 2 relating to a high-risk AI system have been fulfilled"@en ;
    skos:inScheme eu-aiact:assessment-classes ;
    skos:prefLabel "Conformity Assessment"@en .

eu-aiact:ConformityAssessmentBody a rdfs:Class,
        skos:Concept ;
    dct:contributor _:person-delaram-golpayegani ;
    dct:created "2024-04-10"^^xsd:date ;
    dct:source "AIA(Art. 3(21))"@en ;
    rdfs:isDefinedBy eu-aiact: ;
    rdfs:subClassOf tech:Auditor ;
    sw:term_status "accepted"@en ;
    skos:broader tech:Auditor ;
    skos:definition "A body that performs third-party conformity assessment activities, including testing, certification and inspection"@en ;
    skos:inScheme eu-aiact:roles-classes ;
    skos:prefLabel "Conformity Assessment Body"@en .

eu-aiact:CriticalInfrastructureSector a rdfs:Class,
        skos:Concept,
        dpv:Sector ;
    dct:contributor _:person-delaram-golpayegani,
        _:person-harshvardhan-j-pandit ;
    dct:created "2024-12-01"^^xsd:date ;
    dct:source " Annex III"@en,
        "EU AI Act"@en ;
    rdfs:isDefinedBy eu-aiact: ;
    sw:term_status "accepted"@en ;
    skos:broader dpv:Sector ;
    skos:definition "Sector related to provision and maintenance of critical services"@en ;
    skos:inScheme eu-aiact:sector-classes ;
    skos:prefLabel "Critical Infrastructure Sector"@en .

eu-aiact:DeepFakeGeneration a rdfs:Class,
        skos:Concept,
        tech:Capability ;
    dct:contributor _:person-delaram-golpayegani ;
    dct:created "2024-04-10"^^xsd:date ;
    dct:modified "2025-07-30"^^xsd:date ;
    dct:source "AIA Art. 3(60)"@en ;
    rdfs:isDefinedBy eu-aiact: ;
    sw:term_status "modified"@en ;
    skos:broader ai:BiometricIdentification ;
    skos:definition "Capability to generate or manipulate image, audio or video content that resembles existing persons, objects, places, entities or events and would falsely appear to a person to be authentic or truthful;l"@en ;
    skos:inScheme eu-aiact:capability-classes ;
    skos:prefLabel "Deep Fake Generation"@en .

eu-aiact:DemocraticProcessSector a rdfs:Class,
        skos:Concept,
        dpv:Sector ;
    dct:contributor _:person-delaram-golpayegani,
        _:person-harshvardhan-j-pandit ;
    dct:created "2024-12-01"^^xsd:date ;
    dct:source " Annex III"@en,
        "EU AI Act"@en ;
    rdfs:isDefinedBy eu-aiact: ;
    sw:term_status "accepted"@en ;
    skos:broader dpv:Sector ;
    skos:definition "Sector related to administration of democratic processes"@en ;
    skos:inScheme eu-aiact:sector-classes ;
    skos:prefLabel "Democratic Process Sector"@en .

eu-aiact:DeployerHumanOversightMeasure a rdfs:Class,
        skos:Concept,
        dpv:OrganisationalMeasure ;
    dct:contributor _:person-delaram-golpayegani,
        _:person-harshvardhan-j-pandit ;
    dct:created "2026-02-09"^^xsd:date ;
    dct:source " Art. 14 (3b)"@en,
        "AI Act"@en ;
    rdfs:isDefinedBy eu-aiact: ;
    sw:term_status "accepted"@en ;
    skos:broader dpv:HumanOversight ;
    skos:definition "Human oversight measures  identified by the provider before placing the AI system on the market or putting it into service and that are appropriate to be implemented by the deployer."@en ;
    skos:inScheme eu-aiact:risk-classes ;
    skos:prefLabel "Human Oversight Measure by Deployer"@en .

eu-aiact:DownstreamAIProvider a rdfs:Class,
        skos:Concept ;
    dct:contributor _:person-delaram-golpayegani ;
    dct:created "2024-04-10"^^xsd:date ;
    dct:modified "2025-07-30"^^xsd:date ;
    dct:source "AIA(Art. 3(68))"@en ;
    rdfs:isDefinedBy eu-aiact: ;
    rdfs:subClassOf eu-aiact:AIProvider ;
    sw:term_status "accepted"@en ;
    skos:broader eu-aiact:AIProvider ;
    skos:definition "A provider of an AI system, including a general-purpose AI system, which integrates an AI model, regardless of whether the AI model is provided by themselves and vertically integrated or provided by another entity based on contractual relations."@en ;
    skos:inScheme eu-aiact:roles-classes ;
    skos:prefLabel "Downstream AI Provider"@en .

eu-aiact:EUDeclarationOfConformity a rdfs:Class,
        skos:Concept,
        tech:Documentation ;
    dct:contributor _:person-delaram-golpayegani ;
    dct:created "2024-12-01"^^xsd:date ;
    dct:source "AI Act Art.47"@en ;
    rdfs:isDefinedBy eu-aiact: ;
    sw:term_status "accepted"@en ;
    skos:broader tech:Documentation ;
    skos:definition "Document providing the EU declaration of conformity, as required by the AI Act, Article 47"@en ;
    skos:inScheme eu-aiact:docs-classes ;
    skos:prefLabel "EU Declaration Of Conformity"@en .

eu-aiact:EducationSector a rdfs:Class,
        skos:Concept,
        dpv:Sector ;
    dct:contributor _:person-delaram-golpayegani,
        _:person-harshvardhan-j-pandit ;
    dct:created "2024-12-01"^^xsd:date ;
    dct:source " Annex III"@en,
        "EU AI Act"@en ;
    rdfs:isDefinedBy eu-aiact: ;
    sw:term_status "accepted"@en ;
    skos:broader dpv:Sector ;
    skos:definition "Sector related to education and vocational training at any level and for any profession"@en ;
    skos:inScheme eu-aiact:sector-classes ;
    skos:prefLabel "Education Sector"@en .

eu-aiact:EmotionRecognition a rdfs:Class,
        skos:Concept,
        tech:Capability ;
    dct:contributor _:person-delaram-golpayegani ;
    dct:created "2024-04-10"^^xsd:date ;
    dct:modified "2025-07-30"^^xsd:date ;
    dct:source "AIA Art. 3(39)"@en ;
    rdfs:isDefinedBy eu-aiact: ;
    sw:term_status "modified"@en ;
    skos:broader ai:EmotionRecognition ;
    skos:definition "Capability of a technology to identify or infer emotions or intentions of natural persons (on the basis of their biometric data)"@en ;
    skos:inScheme eu-aiact:capability-classes ;
    skos:prefLabel "Emotion Recognition"@en ;
    skos:related pd:Biometric .

eu-aiact:EmotionRecognitionSystem a rdfs:Class,
        skos:Concept,
        eu-aiact:AISystem ;
    dct:contributor _:person-delaram-golpayegani ;
    dct:created "2024-04-10"^^xsd:date ;
    dct:modified "2025-07-30"^^xsd:date ;
    dct:source "AIA(Art. 3(39))"@en ;
    rdfs:isDefinedBy eu-aiact: ;
    sw:term_status "modified"@en ;
    skos:broader eu-aiact:AISystem ;
    skos:definition "An AI system for the purpose of identifying or inferring emotions or intentions of natural persons on the basis of their biometric data."@en ;
    skos:inScheme eu-aiact:system-classes ;
    skos:prefLabel "Emotion Recognition System"@en ;
    skos:related eu-aiact:EmotionRecognition,
        pd:Biometric .

eu-aiact:EmploymentSector a rdfs:Class,
        skos:Concept,
        dpv:Sector ;
    dct:contributor _:person-delaram-golpayegani,
        _:person-harshvardhan-j-pandit ;
    dct:created "2024-12-01"^^xsd:date ;
    dct:source " Annex III"@en,
        "EU AI Act"@en ;
    rdfs:isDefinedBy eu-aiact: ;
    sw:term_status "accepted"@en ;
    skos:broader dpv:Sector ;
    skos:definition "Sector related to employment including workforce management and self-employment"@en ;
    skos:inScheme eu-aiact:sector-classes ;
    skos:prefLabel "Employment Sector"@en .

eu-aiact:FRIA a rdfs:Class,
        skos:Concept,
        dpv:OrganisationalMeasure ;
    dct:contributor _:person-delaram-golpayegani ;
    dct:created "2024-04-10"^^xsd:date ;
    dct:modified "2024-07-30"^^xsd:date ;
    dct:source "AIA(Art. 27)"@en ;
    rdfs:isDefinedBy eu-aiact: ;
    sw:term_status "modified"@en ;
    skos:broader dpv:Assessment ;
    skos:definition "An assessment undertaken to evaluate how the AI use of an AI system might impact fundamental rights"@en ;
    skos:inScheme eu-aiact:assessment-classes ;
    skos:prefLabel "Fundamental Rights Impact Assessment"@en .

eu-aiact:GPAIModel a rdfs:Class,
        skos:Concept ;
    dct:contributor _:person-delaram-golpayegani ;
    dct:created "2024-04-10"^^xsd:date ;
    dct:modified "2025-07-30"^^xsd:date ;
    dct:source "AIA(Art. 3(63))"@en ;
    rdfs:isDefinedBy eu-aiact: ;
    rdfs:subClassOf ai:Model ;
    sw:term_status "modified"@en ;
    skos:broader ai:Model ;
    skos:definition "An AI model, including where such an AI model is trained with a large amount of data using self-supervision at scale, that displays significant generality and is capable of competently performing a wide range of distinct tasks regardless of the way the model is placed on the market and that can be integrated into a variety of downstream systems or applications, except AI models that are used for research, development or prototyping activities before they are placed on the market"@en ;
    skos:inScheme eu-aiact:system-classes ;
    skos:prefLabel "General Purpose AI Model"@en .

eu-aiact:GPAISystem a rdfs:Class,
        skos:Concept ;
    dct:contributor _:person-delaram-golpayegani ;
    dct:created "2024-04-10"^^xsd:date ;
    dct:modified "2025-07-30"^^xsd:date ;
    dct:source "AIA(Art.3 (66))"@en ;
    rdfs:isDefinedBy eu-aiact: ;
    rdfs:subClassOf eu-aiact:AISystem ;
    sw:term_status "modified"@en ;
    skos:broader eu-aiact:AISystem ;
    skos:definition "An AI system which is based on a general-purpose AI model and which has the capability to serve a variety of purposes, both for direct use as well as for integration in other AI systems"@en ;
    skos:inScheme eu-aiact:system-classes ;
    skos:prefLabel "General Purpose AI System"@en .

eu-aiact:HighImpactCapabilityGPAIModel a rdfs:Class,
        skos:Concept,
        tech:Capability ;
    dct:contributor _:person-delaram-golpayegani ;
    dct:created "2024-04-10"^^xsd:date ;
    dct:modified "2025-07-30"^^xsd:date ;
    dct:source "AIA Art. 3(64)"@en ;
    rdfs:isDefinedBy eu-aiact: ;
    sw:term_status "modified"@en ;
    skos:broader tech:Capability ;
    skos:definition "‘High-impact Capabilities’ in general purpose AI models means capabilities that match or exceed the capabilities recorded in the most advanced general purpose AI models"@en ;
    skos:inScheme eu-aiact:capability-classes ;
    skos:prefLabel "High-Impact Capability in General Purpose AI Models"@en .

eu-aiact:HighRiskAIAssessment a rdfs:Class,
        skos:Concept,
        dpv:OrganisationalMeasure ;
    dct:contributor _:person-delaram-golpayegani ;
    dct:created "2024-04-10"^^xsd:date ;
    dct:modified "2024-07-30"^^xsd:date ;
    dct:source "AIA(Art. 6)"@en ;
    rdfs:isDefinedBy eu-aiact: ;
    sw:term_status "modified"@en ;
    skos:broader dpv:Assessment ;
    skos:definition "An assessment undertaken to determine whether the AI system is classified as high-risk under the AI Act"@en ;
    skos:inScheme eu-aiact:assessment-classes ;
    skos:prefLabel "High Risk AI Assessment"@en .

eu-aiact:HighRiskAISystem a rdfs:Class,
        skos:Concept ;
    dct:contributor _:person-delaram-golpayegani,
        _:person-harshvardhan-j-pandit ;
    dct:created "2026-02-09"^^xsd:date ;
    dct:source "AIA(Art.6)"@en ;
    rdfs:isDefinedBy eu-aiact: ;
    rdfs:subClassOf eu-aiact:AISystem ;
    sw:term_status "accepted"@en ;
    skos:broader eu-aiact:AISystem ;
    skos:definition "High-risk AI system according to the AI Act"@en ;
    skos:inScheme eu-aiact:system-classes ;
    skos:prefLabel "High Risk AI System"@en .

eu-aiact:HighRiskAISystem-A6-1 a rdfs:Class,
        skos:Concept ;
    dct:contributor _:person-delaram-golpayegani,
        _:person-harshvardhan-j-pandit ;
    dct:created "2026-02-09"^^xsd:date ;
    dct:source "AIA(Art.6(1))"@en ;
    rdfs:isDefinedBy eu-aiact: ;
    rdfs:subClassOf eu-aiact:HighRiskAISystem ;
    sw:term_status "accepted"@en ;
    skos:broader eu-aiact:HighRiskAISystem ;
    skos:definition "High-risk AI system according to Article 6(1) of the AI Act which refers to sectorial laws in Annex I"@en ;
    skos:inScheme eu-aiact:highrisk-systems-classes ;
    skos:prefLabel "High Risk AI System per Article 6(1)"@en ;
    eu-aiact:hasRiskLevel eu-aiact:RiskLevelHigh-A6-1 .

eu-aiact:HighRiskAISystem-A6-2 a rdfs:Class,
        skos:Concept ;
    dct:contributor _:person-delaram-golpayegani,
        _:person-harshvardhan-j-pandit ;
    dct:created "2026-02-09"^^xsd:date ;
    dct:source "AIA(Art.6(2))"@en ;
    rdfs:isDefinedBy eu-aiact: ;
    rdfs:subClassOf eu-aiact:HighRiskAISystem ;
    sw:term_status "accepted"@en ;
    skos:broader eu-aiact:HighRiskAISystem ;
    skos:definition "High-risk AI system according to Article 6(2) of the AI Act which refers to specific applications in Annex III"@en ;
    skos:inScheme eu-aiact:highrisk-systems-classes ;
    skos:prefLabel "High Risk AI System per Article 6(2)"@en ;
    eu-aiact:hasRiskLevel eu-aiact:RiskLevelHigh-A6-2 .

eu-aiact:HighRiskAISystem-AnnexI-1 a rdfs:Class,
        skos:Concept,
        eu-aiact:HighRiskAISystem ;
    dct:contributor _:person-delaram-golpayegani,
        _:person-harshvardhan-j-pandit ;
    dct:created "2026-02-09"^^xsd:date ;
    dct:source "AIA(Anx.I)"@en ;
    rdfs:isDefinedBy eu-aiact: ;
    sw:term_status "accepted"@en ;
    skos:broader eu-aiact:HighRiskAISystem-A6-1 ;
    skos:definition "High-risk AI system according to Annex I, point 1: AI system that is intended to be used as a safety component of a product, or the AI system is itself a product, covered by Directive 2006/42/EC of the European Parliament and of the Council of 17 May 2006 on machinery, and amending Directive 95/16/EC (OJ L 157, 9.6.2006, p. 24)"@en ;
    skos:inScheme eu-aiact:highrisk-systems-classes ;
    skos:prefLabel "High-Risk AI System - Annex I(1)"@en ;
    eu-aiact:hasRiskLevel eu-aiact:RiskLevelHigh-A6-1 .

eu-aiact:HighRiskAISystem-AnnexI-10 a rdfs:Class,
        skos:Concept,
        eu-aiact:HighRiskAISystem ;
    dct:contributor _:person-delaram-golpayegani,
        _:person-harshvardhan-j-pandit ;
    dct:created "2026-02-09"^^xsd:date ;
    dct:source "AIA(Anx.I)"@en ;
    rdfs:isDefinedBy eu-aiact: ;
    sw:term_status "accepted"@en ;
    skos:broader eu-aiact:HighRiskAISystem-A6-1 ;
    skos:definition """High-risk AI system according to Annex I, point 10: AI system that is intended to be used as a safety component of a product, or the AI system is itself a product, covered by 
Regulation (EU) 2016/426 of the European Parliament and of the Council of 9 March 2016 on appliances burning gaseous fuels and repealing Directive 2009/142/EC (OJ L 81, 31.3.2016, p. 99)"""@en ;
    skos:inScheme eu-aiact:highrisk-systems-classes ;
    skos:prefLabel "High-Risk AI System - Annex I(10)"@en ;
    eu-aiact:hasRiskLevel eu-aiact:RiskLevelHigh-A6-1 .

eu-aiact:HighRiskAISystem-AnnexI-11 a rdfs:Class,
        skos:Concept,
        eu-aiact:HighRiskAISystem ;
    dct:contributor _:person-delaram-golpayegani,
        _:person-harshvardhan-j-pandit ;
    dct:created "2026-02-09"^^xsd:date ;
    dct:source "AIA(Anx.I)"@en ;
    rdfs:isDefinedBy eu-aiact: ;
    sw:term_status "accepted"@en ;
    skos:broader eu-aiact:HighRiskAISystem-A6-1 ;
    skos:definition """High-risk AI system according to Annex I, point 11: AI system that is intended to be used as a safety component of a product, or the AI system is itself a product, covered by 
Regulation (EU) 2017/745 of the European Parliament and of the Council of 5 April 2017 on medical devices, amending Directive 2001/83/EC, Regulation (EC) No 178/2002 and Regulation (EC) No 1223/2009 and repealing Council Directives 90/385/EEC and 93/42/EEC (OJ L 117, 5.5.2017, p. 1)"""@en ;
    skos:inScheme eu-aiact:highrisk-systems-classes ;
    skos:prefLabel "High-Risk AI System - Annex I(11)"@en ;
    eu-aiact:hasRiskLevel eu-aiact:RiskLevelHigh-A6-1 .

eu-aiact:HighRiskAISystem-AnnexI-12 a rdfs:Class,
        skos:Concept,
        eu-aiact:HighRiskAISystem ;
    dct:contributor _:person-delaram-golpayegani,
        _:person-harshvardhan-j-pandit ;
    dct:created "2026-02-09"^^xsd:date ;
    dct:source "AIA(Anx.I)"@en ;
    rdfs:isDefinedBy eu-aiact: ;
    sw:term_status "accepted"@en ;
    skos:broader eu-aiact:HighRiskAISystem-A6-1 ;
    skos:definition """High-risk AI system according to Annex I, point 12: AI system that is intended to be used as a safety component of a product, or the AI system is itself a product, covered by 
Regulation (EU) 2017/746 of the European Parliament and of the Council of 5 April 2017 on in vitro diagnostic medical devices and repealing Directive 98/79/EC and Commission Decision 2010/227/EU (OJ L 117, 5.5.2017, p. 176)"""@en ;
    skos:inScheme eu-aiact:highrisk-systems-classes ;
    skos:prefLabel "High-Risk AI System - Annex I(12)"@en ;
    eu-aiact:hasRiskLevel eu-aiact:RiskLevelHigh-A6-1 .

eu-aiact:HighRiskAISystem-AnnexI-13 a rdfs:Class,
        skos:Concept,
        eu-aiact:HighRiskAISystem ;
    dct:contributor _:person-delaram-golpayegani,
        _:person-harshvardhan-j-pandit ;
    dct:created "2026-02-09"^^xsd:date ;
    dct:source "AIA(Anx.I)"@en ;
    rdfs:isDefinedBy eu-aiact: ;
    sw:term_status "accepted"@en ;
    skos:broader eu-aiact:HighRiskAISystem-A6-1 ;
    skos:definition """High-risk AI system according to Annex I, point 13: AI system that is intended to be used as a safety component of a product, or the AI system is itself a product, covered by 
Regulation (EC) No 300/2008 of the European Parliament and of the Council of 11 March 2008 on common rules in the field of civil aviation security and repealing Regulation (EC) No 2320/2002 (OJ L 97, 9.4.2008, p. 72)"""@en ;
    skos:inScheme eu-aiact:highrisk-systems-classes ;
    skos:prefLabel "High-Risk AI System - Annex I(13)"@en ;
    eu-aiact:hasRiskLevel eu-aiact:RiskLevelHigh-A6-1 .

eu-aiact:HighRiskAISystem-AnnexI-14 a rdfs:Class,
        skos:Concept,
        eu-aiact:HighRiskAISystem ;
    dct:contributor _:person-delaram-golpayegani,
        _:person-harshvardhan-j-pandit ;
    dct:created "2026-02-09"^^xsd:date ;
    dct:source "AIA(Anx.I)"@en ;
    rdfs:isDefinedBy eu-aiact: ;
    sw:term_status "accepted"@en ;
    skos:broader eu-aiact:HighRiskAISystem-A6-1 ;
    skos:definition """High-risk AI system according to Annex I, point 14: AI system that is intended to be used as a safety component of a product, or the AI system is itself a product, covered by 
Regulation (EU) No 168/2013 of the European Parliament and of the Council of 15 January 2013 on the approval and market surveillance of two- or three-wheel vehicles and quadricycles (OJ L 60, 2.3.2013, p. 52)"""@en ;
    skos:inScheme eu-aiact:highrisk-systems-classes ;
    skos:prefLabel "High-Risk AI System - Annex I(14)"@en ;
    eu-aiact:hasRiskLevel eu-aiact:RiskLevelHigh-A6-1 .

eu-aiact:HighRiskAISystem-AnnexI-15 a rdfs:Class,
        skos:Concept,
        eu-aiact:HighRiskAISystem ;
    dct:contributor _:person-delaram-golpayegani,
        _:person-harshvardhan-j-pandit ;
    dct:created "2026-02-09"^^xsd:date ;
    dct:source "AIA(Anx.I)"@en ;
    rdfs:isDefinedBy eu-aiact: ;
    sw:term_status "accepted"@en ;
    skos:broader eu-aiact:HighRiskAISystem-A6-1 ;
    skos:definition """High-risk AI system according to Annex I, point 15: AI system that is intended to be used as a safety component of a product, or the AI system is itself a product, covered by 
Regulation (EU) No 167/2013 of the European Parliament and of the Council of 5 February 2013 on the approval and market surveillance of agricultural and forestry vehicles (OJ L 60, 2.3.2013, p. 1)"""@en ;
    skos:inScheme eu-aiact:highrisk-systems-classes ;
    skos:prefLabel "High-Risk AI System - Annex I(15)"@en ;
    eu-aiact:hasRiskLevel eu-aiact:RiskLevelHigh-A6-1 .

eu-aiact:HighRiskAISystem-AnnexI-16 a rdfs:Class,
        skos:Concept,
        eu-aiact:HighRiskAISystem ;
    dct:contributor _:person-delaram-golpayegani,
        _:person-harshvardhan-j-pandit ;
    dct:created "2026-02-09"^^xsd:date ;
    dct:source "AIA(Anx.I)"@en ;
    rdfs:isDefinedBy eu-aiact: ;
    sw:term_status "accepted"@en ;
    skos:broader eu-aiact:HighRiskAISystem-A6-1 ;
    skos:definition """High-risk AI system according to Annex I, point 16: AI system that is intended to be used as a safety component of a product, or the AI system is itself a product, covered by 
Directive 2014/90/EU of the European Parliament and of the Council of 23 July 2014 on marine equipment and repealing Council Directive 96/98/EC (OJ L 257, 28.8.2014, p. 146)"""@en ;
    skos:inScheme eu-aiact:highrisk-systems-classes ;
    skos:prefLabel "High-Risk AI System - Annex I(16)"@en ;
    eu-aiact:hasRiskLevel eu-aiact:RiskLevelHigh-A6-1 .

eu-aiact:HighRiskAISystem-AnnexI-17 a rdfs:Class,
        skos:Concept,
        eu-aiact:HighRiskAISystem ;
    dct:contributor _:person-delaram-golpayegani,
        _:person-harshvardhan-j-pandit ;
    dct:created "2026-02-09"^^xsd:date ;
    dct:source "AIA(Anx.I)"@en ;
    rdfs:isDefinedBy eu-aiact: ;
    sw:term_status "accepted"@en ;
    skos:broader eu-aiact:HighRiskAISystem-A6-1 ;
    skos:definition """High-risk AI system according to Annex I, point 17: AI system that is intended to be used as a safety component of a product, or the AI system is itself a product, covered by 
Directive (EU) 2016/797 of the European Parliament and of the Council of 11 May 2016 on the interoperability of the rail system within the European Union (OJ L 138, 26.5.2016, p. 44)"""@en ;
    skos:inScheme eu-aiact:highrisk-systems-classes ;
    skos:prefLabel "High-Risk AI System - Annex I(17)"@en ;
    eu-aiact:hasRiskLevel eu-aiact:RiskLevelHigh-A6-1 .

eu-aiact:HighRiskAISystem-AnnexI-18 a rdfs:Class,
        skos:Concept,
        eu-aiact:HighRiskAISystem ;
    dct:contributor _:person-delaram-golpayegani,
        _:person-harshvardhan-j-pandit ;
    dct:created "2026-02-09"^^xsd:date ;
    dct:source "AIA(Anx.I)"@en ;
    rdfs:isDefinedBy eu-aiact: ;
    sw:term_status "accepted"@en ;
    skos:broader eu-aiact:HighRiskAISystem-A6-1 ;
    skos:definition """High-risk AI system according to Annex I, point 18: AI system that is intended to be used as a safety component of a product, or the AI system is itself a product, covered by 
Regulation (EU) 2018/858 of the European Parliament and of the Council of 30 May 2018 on the approval and market surveillance of motor vehicles and their trailers, and of systems, components and separate technical units intended for such vehicles, amending Regulations (EC) No 715/2007 and (EC) No 595/2009 and repealing Directive 2007/46/EC (OJ L 151, 14.6.2018, p. 1)"""@en ;
    skos:inScheme eu-aiact:highrisk-systems-classes ;
    skos:prefLabel "High-Risk AI System - Annex I(18)"@en ;
    eu-aiact:hasRiskLevel eu-aiact:RiskLevelHigh-A6-1 .

eu-aiact:HighRiskAISystem-AnnexI-19 a rdfs:Class,
        skos:Concept,
        eu-aiact:HighRiskAISystem ;
    dct:contributor _:person-delaram-golpayegani,
        _:person-harshvardhan-j-pandit ;
    dct:created "2026-02-09"^^xsd:date ;
    dct:source "AIA(Anx.I)"@en ;
    rdfs:isDefinedBy eu-aiact: ;
    sw:term_status "accepted"@en ;
    skos:broader eu-aiact:HighRiskAISystem-A6-1 ;
    skos:definition """High-risk AI system according to Annex I, point 19: AI system that is intended to be used as a safety component of a product, or the AI system is itself a product, covered by 
Regulation (EU) 2019/2144 of the European Parliament and of the Council of 27 November 2019 on type-approval requirements for motor vehicles and their trailers, and systems, components and separate technical units intended for such vehicles, as regards their general safety and the protection of vehicle occupants and vulnerable road users, amending Regulation (EU) 2018/858 of the European Parliament and of the Council and repealing Regulations (EC) No 78/2009, (EC) No 79/2009 and (EC) No 661/2009 of the European Parliament and of the Council and Commission Regulations (EC) No 631/2009, (EU) No 406/2010, (EU) No 672/2010, (EU) No 1003/2010, (EU) No 1005/2010, (EU) No 1008/2010, (EU) No 1009/2010, (EU) No 19/2011, (EU) No 109/2011, (EU) No 458/2011, (EU) No 65/2012, (EU) No 130/2012, (EU) No 347/2012, (EU) No 351/2012, (EU) No 1230/2012 and (EU) 2015/166 (OJ L 325, 16.12.2019, p. 1)"""@en ;
    skos:inScheme eu-aiact:highrisk-systems-classes ;
    skos:prefLabel "High-Risk AI System - Annex I(19)"@en ;
    eu-aiact:hasRiskLevel eu-aiact:RiskLevelHigh-A6-1 .

eu-aiact:HighRiskAISystem-AnnexI-2 a rdfs:Class,
        skos:Concept,
        eu-aiact:HighRiskAISystem ;
    dct:contributor _:person-delaram-golpayegani,
        _:person-harshvardhan-j-pandit ;
    dct:created "2026-02-09"^^xsd:date ;
    dct:source "AIA(Anx.I)"@en ;
    rdfs:isDefinedBy eu-aiact: ;
    sw:term_status "accepted"@en ;
    skos:broader eu-aiact:HighRiskAISystem-A6-1 ;
    skos:definition "High-risk AI system according to Annex I, point 2: AI system that is intended to be used as a safety component of a product, or the AI system is itself a product, covered by Directive 2009/48/EC of the European Parliament and of the Council of 18 June 2009 on the safety of toys (OJ L 170, 30.6.2009, p. 1)"@en ;
    skos:inScheme eu-aiact:highrisk-systems-classes ;
    skos:prefLabel "High-Risk AI System - Annex I(2)"@en ;
    eu-aiact:hasRiskLevel eu-aiact:RiskLevelHigh-A6-1 .

eu-aiact:HighRiskAISystem-AnnexI-20 a rdfs:Class,
        skos:Concept,
        eu-aiact:HighRiskAISystem ;
    dct:contributor _:person-delaram-golpayegani,
        _:person-harshvardhan-j-pandit ;
    dct:created "2026-02-09"^^xsd:date ;
    dct:source "AIA(Anx.I)"@en ;
    rdfs:isDefinedBy eu-aiact: ;
    sw:term_status "accepted"@en ;
    skos:broader eu-aiact:HighRiskAISystem-A6-1 ;
    skos:definition """High-risk AI system according to Annex I, point 20: AI system that is intended to be used as a safety component of a product, or the AI system is itself a product, covered by 
Regulation (EU) 2018/1139 of the European Parliament and of the Council of 4 July 2018 on common rules in the field of civil aviation and establishing a European Union Aviation Safety Agency, and amending Regulations (EC) No 2111/2005, (EC) No 1008/2008, (EU) No 996/2010, (EU) No 376/2014 and Directives 2014/30/EU and 2014/53/EU of the European Parliament and of the Council, and repealing Regulations (EC) No 552/2004 and (EC) No 216/2008 of the European Parliament and of the Council and Council Regulation (EEC) No 3922/91 (OJ L 212, 22.8.2018, p. 1), in so far as the design, production and placing on the market of aircrafts referred to in Article 2(1), points (a) and (b) thereof, where it concerns unmanned aircraft and their engines, propellers, parts and equipment to control them remotely, are concerned."""@en ;
    skos:inScheme eu-aiact:highrisk-systems-classes ;
    skos:prefLabel "High-Risk AI System - Annex I(20)"@en ;
    eu-aiact:hasRiskLevel eu-aiact:RiskLevelHigh-A6-1 .

eu-aiact:HighRiskAISystem-AnnexI-3 a rdfs:Class,
        skos:Concept,
        eu-aiact:HighRiskAISystem ;
    dct:contributor _:person-delaram-golpayegani,
        _:person-harshvardhan-j-pandit ;
    dct:created "2026-02-09"^^xsd:date ;
    dct:source "AIA(Anx.I)"@en ;
    rdfs:isDefinedBy eu-aiact: ;
    sw:term_status "accepted"@en ;
    skos:broader eu-aiact:HighRiskAISystem-A6-1 ;
    skos:definition "High-risk AI system according to Annex I, point 3: AI system that is intended to be used as a safety component of a product, or the AI system is itself a product, covered by Directive 2013/53/EU of the European Parliament and of the Council of 20 November 2013 on recreational craft and personal watercraft and repealing Directive 94/25/EC (OJ L 354, 28.12.2013, p. 90);"@en ;
    skos:inScheme eu-aiact:highrisk-systems-classes ;
    skos:prefLabel "High-Risk AI System - Annex I(3)"@en ;
    eu-aiact:hasRiskLevel eu-aiact:RiskLevelHigh-A6-1 .

eu-aiact:HighRiskAISystem-AnnexI-4 a rdfs:Class,
        skos:Concept,
        eu-aiact:HighRiskAISystem ;
    dct:contributor _:person-delaram-golpayegani,
        _:person-harshvardhan-j-pandit ;
    dct:created "2026-02-09"^^xsd:date ;
    dct:source "AIA(Anx.I)"@en ;
    rdfs:isDefinedBy eu-aiact: ;
    sw:term_status "accepted"@en ;
    skos:broader eu-aiact:HighRiskAISystem-A6-1 ;
    skos:definition "High-risk AI system according to Annex I, point 4: AI system that is intended to be used as a safety component of a product, or the AI system is itself a product, covered by Directive 2014/33/EU of the European Parliament and of the Council of 26 February 2014 on the harmonisation of the laws of the Member States relating to lifts and safety components for lifts (OJ L 96, 29.3.2014, p. 251)"@en ;
    skos:inScheme eu-aiact:highrisk-systems-classes ;
    skos:prefLabel "High-Risk AI System - Annex I(4)"@en ;
    eu-aiact:hasRiskLevel eu-aiact:RiskLevelHigh-A6-1 .

eu-aiact:HighRiskAISystem-AnnexI-5 a rdfs:Class,
        skos:Concept,
        eu-aiact:HighRiskAISystem ;
    dct:contributor _:person-delaram-golpayegani,
        _:person-harshvardhan-j-pandit ;
    dct:created "2026-02-09"^^xsd:date ;
    dct:source "AIA(Anx.I)"@en ;
    rdfs:isDefinedBy eu-aiact: ;
    sw:term_status "accepted"@en ;
    skos:broader eu-aiact:HighRiskAISystem-A6-1 ;
    skos:definition "High-risk AI system according to Annex I, point 5: AI system that is intended to be used as a safety component of a product, or the AI system is itself a product, covered by Directive 2014/34/EU of the European Parliament and of the Council of 26 February 2014 on the harmonisation of the laws of the Member States relating to equipment and protective systems intended for use in potentially explosive atmospheres (OJ L 96, 29.3.2014, p. 309);"@en ;
    skos:inScheme eu-aiact:highrisk-systems-classes ;
    skos:prefLabel "High-Risk AI System - Annex I(5)"@en ;
    eu-aiact:hasRiskLevel eu-aiact:RiskLevelHigh-A6-1 .

eu-aiact:HighRiskAISystem-AnnexI-6 a rdfs:Class,
        skos:Concept,
        eu-aiact:HighRiskAISystem ;
    dct:contributor _:person-delaram-golpayegani,
        _:person-harshvardhan-j-pandit ;
    dct:created "2026-02-09"^^xsd:date ;
    dct:source "AIA(Anx.I)"@en ;
    rdfs:isDefinedBy eu-aiact: ;
    sw:term_status "accepted"@en ;
    skos:broader eu-aiact:HighRiskAISystem-A6-1 ;
    skos:definition "High-risk AI system according to Annex I, point 6: AI system that is intended to be used as a safety component of a product, or the AI system is itself a product, covered by Directive 2014/53/EU of the European Parliament and of the Council of 16 April 2014 on the harmonisation of the laws of the Member States relating to the making available on the market of radio equipment and repealing Directive 1999/5/EC (OJ L 153, 22.5.2014, p. 62)"@en ;
    skos:inScheme eu-aiact:highrisk-systems-classes ;
    skos:prefLabel "High-Risk AI System - Annex I(6)"@en ;
    eu-aiact:hasRiskLevel eu-aiact:RiskLevelHigh-A6-1 .

eu-aiact:HighRiskAISystem-AnnexI-7 a rdfs:Class,
        skos:Concept,
        eu-aiact:HighRiskAISystem ;
    dct:contributor _:person-delaram-golpayegani,
        _:person-harshvardhan-j-pandit ;
    dct:created "2026-02-09"^^xsd:date ;
    dct:source "AIA(Anx.I)"@en ;
    rdfs:isDefinedBy eu-aiact: ;
    sw:term_status "accepted"@en ;
    skos:broader eu-aiact:HighRiskAISystem-A6-1 ;
    skos:definition "High-risk AI system according to Annex I, point 7: AI system that is intended to be used as a safety component of a product, or the AI system is itself a product, covered by  Directive 2014/68/EU of the European Parliament and of the Council of 15 May 2014 on the harmonisation of the laws of the Member States relating to the making available on the market of pressure equipment (OJ L 189, 27.6.2014, p. 164)"@en ;
    skos:inScheme eu-aiact:highrisk-systems-classes ;
    skos:prefLabel "High-Risk AI System - Annex I(7)"@en ;
    eu-aiact:hasRiskLevel eu-aiact:RiskLevelHigh-A6-1 .

eu-aiact:HighRiskAISystem-AnnexI-8 a rdfs:Class,
        skos:Concept,
        eu-aiact:HighRiskAISystem ;
    dct:contributor _:person-delaram-golpayegani,
        _:person-harshvardhan-j-pandit ;
    dct:created "2026-02-09"^^xsd:date ;
    dct:source "AIA(Anx.I)"@en ;
    rdfs:isDefinedBy eu-aiact: ;
    sw:term_status "accepted"@en ;
    skos:broader eu-aiact:HighRiskAISystem-A6-1 ;
    skos:definition "High-risk AI system according to Annex I, point 8: AI system that is intended to be used as a safety component of a product, or the AI system is itself a product, covered by Regulation (EU) 2016/424 of the European Parliament and of the Council of 9 March 2016 on cableway installations and repealing Directive 2000/9/EC (OJ L 81, 31.3.2016, p. 1)"@en ;
    skos:inScheme eu-aiact:highrisk-systems-classes ;
    skos:prefLabel "High-Risk AI System - Annex I(8)"@en ;
    eu-aiact:hasRiskLevel eu-aiact:RiskLevelHigh-A6-1 .

eu-aiact:HighRiskAISystem-AnnexI-9 a rdfs:Class,
        skos:Concept,
        eu-aiact:HighRiskAISystem ;
    dct:contributor _:person-delaram-golpayegani,
        _:person-harshvardhan-j-pandit ;
    dct:created "2026-02-09"^^xsd:date ;
    dct:source "AIA(Anx.I)"@en ;
    rdfs:isDefinedBy eu-aiact: ;
    sw:term_status "accepted"@en ;
    skos:broader eu-aiact:HighRiskAISystem-A6-1 ;
    skos:definition """High-risk AI system according to Annex I, point 9: AI system that is intended to be used as a safety component of a product, or the AI system is itself a product, covered by 
Regulation (EU) 2016/425 of the European Parliament and of the Council of 9 March 2016 on personal protective equipment and repealing Council Directive 89/686/EEC (OJ L 81, 31.3.2016, p. 51)"""@en ;
    skos:inScheme eu-aiact:highrisk-systems-classes ;
    skos:prefLabel "High-Risk AI System - Annex I(9)"@en ;
    eu-aiact:hasRiskLevel eu-aiact:RiskLevelHigh-A6-1 .

eu-aiact:HighRiskAISystem-AnnexIII-1-a a rdfs:Class,
        skos:Concept,
        eu-aiact:HighRiskAISystem ;
    dct:contributor _:person-delaram-golpayegani,
        _:person-harshvardhan-j-pandit ;
    dct:created "2026-02-09"^^xsd:date ;
    dct:source "AIA(Anx.III)"@en ;
    rdfs:isDefinedBy eu-aiact: ;
    sw:term_status "accepted"@en ;
    skos:broader eu-aiact:HighRiskAISystem-A6-2 ;
    skos:definition "High-risk AI system according to Annex III, Point 1a:  Biometrics, remote biometric identification systems. This shall not include AI systems intended to be used for biometric verification the sole purpose of which is to confirm that a specific natural person is the person he or she claims to be."@en ;
    skos:inScheme eu-aiact:highrisk-systems-classes ;
    skos:prefLabel "High-Risk AI System - Annex III(1a)"@en ;
    eu-aiact:hasRiskLevel eu-aiact:RiskLevelHigh-A6-2 .

eu-aiact:HighRiskAISystem-AnnexIII-1-b a rdfs:Class,
        skos:Concept,
        eu-aiact:HighRiskAISystem ;
    dct:contributor _:person-delaram-golpayegani,
        _:person-harshvardhan-j-pandit ;
    dct:created "2026-02-09"^^xsd:date ;
    dct:source "AIA(Anx.III)"@en ;
    rdfs:isDefinedBy eu-aiact: ;
    sw:term_status "accepted"@en ;
    skos:broader eu-aiact:HighRiskAISystem-A6-2 ;
    skos:definition "High-risk AI system according to Annex III, Point 1b:  Biometrics, AI systems intended to be used for biometric categorisation, according to sensitive or protected attributes or characteristics based on the inference of those attributes or characteristics."@en ;
    skos:inScheme eu-aiact:highrisk-systems-classes ;
    skos:prefLabel "High-Risk AI System - Annex III(1b)"@en ;
    eu-aiact:hasRiskLevel eu-aiact:RiskLevelHigh-A6-2 .

eu-aiact:HighRiskAISystem-AnnexIII-1-c a rdfs:Class,
        skos:Concept,
        eu-aiact:HighRiskAISystem ;
    dct:contributor _:person-delaram-golpayegani,
        _:person-harshvardhan-j-pandit ;
    dct:created "2026-02-09"^^xsd:date ;
    dct:source "AIA(Anx.III)"@en ;
    rdfs:isDefinedBy eu-aiact: ;
    sw:term_status "accepted"@en ;
    skos:broader eu-aiact:HighRiskAISystem-A6-2 ;
    skos:definition "High-risk AI system according to Annex III, Point 1c:  Biometrics, AI systems intended to be used for emotion recognition."@en ;
    skos:inScheme eu-aiact:highrisk-systems-classes ;
    skos:prefLabel "High-Risk AI System - Annex III(1c)"@en ;
    eu-aiact:hasRiskLevel eu-aiact:RiskLevelHigh-A6-2 .

eu-aiact:HighRiskAISystem-AnnexIII-2 a rdfs:Class,
        skos:Concept,
        eu-aiact:HighRiskAISystem ;
    dct:contributor _:person-delaram-golpayegani,
        _:person-harshvardhan-j-pandit ;
    dct:created "2026-02-09"^^xsd:date ;
    dct:source "AIA(Anx.III)"@en ;
    rdfs:isDefinedBy eu-aiact: ;
    sw:term_status "accepted"@en ;
    skos:broader eu-aiact:HighRiskAISystem-A6-2 ;
    skos:definition "High-risk AI system according to Annex III, Point 2: Critical infrastructure: AI systems intended to be used as safety components in the management and operation of critical digital infrastructure, road traffic, or in the supply of water, gas, heating or electricity"@en ;
    skos:inScheme eu-aiact:highrisk-systems-classes ;
    skos:prefLabel "High-Risk AI System - Annex III(2)"@en ;
    eu-aiact:hasRiskLevel eu-aiact:RiskLevelHigh-A6-2 .

eu-aiact:HighRiskAISystem-AnnexIII-3-a a rdfs:Class,
        skos:Concept,
        eu-aiact:HighRiskAISystem ;
    dct:contributor _:person-delaram-golpayegani,
        _:person-harshvardhan-j-pandit ;
    dct:created "2026-02-09"^^xsd:date ;
    dct:source "AIA(Anx.III)"@en ;
    rdfs:isDefinedBy eu-aiact: ;
    sw:term_status "accepted"@en ;
    skos:broader eu-aiact:HighRiskAISystem-A6-2 ;
    skos:definition "High-risk AI system according to Annex III, Point 3a: AI systems intended to be used to determine access or admission or to assign natural persons to educational and vocational training institutions at all levels;"@en ;
    skos:inScheme eu-aiact:highrisk-systems-classes ;
    skos:prefLabel "High-Risk AI System - Annex III(3a)"@en ;
    eu-aiact:hasRiskLevel eu-aiact:RiskLevelHigh-A6-2 .

eu-aiact:HighRiskAISystem-AnnexIII-3-b a rdfs:Class,
        skos:Concept,
        eu-aiact:HighRiskAISystem ;
    dct:contributor _:person-delaram-golpayegani,
        _:person-harshvardhan-j-pandit ;
    dct:created "2026-02-09"^^xsd:date ;
    dct:source "AIA(Anx.III)"@en ;
    rdfs:isDefinedBy eu-aiact: ;
    sw:term_status "accepted"@en ;
    skos:broader eu-aiact:HighRiskAISystem-A6-2 ;
    skos:definition "High-risk AI system according to Annex III, Point 3b: Education and vocational training: AI systems intended to be used to evaluate learning outcomes, including when those outcomes are used to steer the learning process of natural persons in educational and vocational training institutions at all levels"@en ;
    skos:inScheme eu-aiact:highrisk-systems-classes ;
    skos:prefLabel "High-Risk AI System - Annex III(3b)"@en ;
    eu-aiact:hasRiskLevel eu-aiact:RiskLevelHigh-A6-2 .

eu-aiact:HighRiskAISystem-AnnexIII-3-c a rdfs:Class,
        skos:Concept,
        eu-aiact:HighRiskAISystem ;
    dct:contributor _:person-delaram-golpayegani,
        _:person-harshvardhan-j-pandit ;
    dct:created "2026-02-09"^^xsd:date ;
    dct:source "AIA(Anx.III)"@en ;
    rdfs:isDefinedBy eu-aiact: ;
    sw:term_status "accepted"@en ;
    skos:broader eu-aiact:HighRiskAISystem-A6-2 ;
    skos:definition "High-risk AI system according to Annex III, Point 3c: Education and vocational training: AI systems intended to be used for the purpose of assessing the appropriate level of education that an individual will receive or will be able to access, in the context of or within educational and vocational training institutions at all levels"@en ;
    skos:inScheme eu-aiact:highrisk-systems-classes ;
    skos:prefLabel "High-Risk AI System - Annex III(3c)"@en ;
    eu-aiact:hasRiskLevel eu-aiact:RiskLevelHigh-A6-2 .

eu-aiact:HighRiskAISystem-AnnexIII-3-d a rdfs:Class,
        skos:Concept,
        eu-aiact:HighRiskAISystem ;
    dct:contributor _:person-delaram-golpayegani,
        _:person-harshvardhan-j-pandit ;
    dct:created "2026-02-09"^^xsd:date ;
    dct:source "AIA(Anx.III)"@en ;
    rdfs:isDefinedBy eu-aiact: ;
    sw:term_status "accepted"@en ;
    skos:broader eu-aiact:HighRiskAISystem-A6-2 ;
    skos:definition "High-risk AI system according to Annex III, Point 3d: Education and vocational training: AI systems intended to be used for monitoring and detecting prohibited behaviour of students during tests in the context of or within educational and vocational training institutions at all levels"@en ;
    skos:inScheme eu-aiact:highrisk-systems-classes ;
    skos:prefLabel "High-Risk AI System - Annex III(3d)"@en ;
    eu-aiact:hasRiskLevel eu-aiact:RiskLevelHigh-A6-2 .

eu-aiact:HighRiskAISystem-AnnexIII-4-a a rdfs:Class,
        skos:Concept,
        eu-aiact:HighRiskAISystem ;
    dct:contributor _:person-delaram-golpayegani,
        _:person-harshvardhan-j-pandit ;
    dct:created "2026-02-09"^^xsd:date ;
    dct:source "AIA(Anx.III)"@en ;
    rdfs:isDefinedBy eu-aiact: ;
    sw:term_status "accepted"@en ;
    skos:broader eu-aiact:HighRiskAISystem-A6-2 ;
    skos:definition "High-risk AI system according to Annex III, Point 4a: Employment, workers management and access to self-employment: AI systems intended to be used for the recruitment or selection of natural persons, in particular to place targeted job advertisements, to analyse and filter job applications, and to evaluate candidates"@en ;
    skos:inScheme eu-aiact:highrisk-systems-classes ;
    skos:prefLabel "High-Risk AI System - Annex III(4a)"@en ;
    eu-aiact:hasRiskLevel eu-aiact:RiskLevelHigh-A6-2 .

eu-aiact:HighRiskAISystem-AnnexIII-4-b a rdfs:Class,
        skos:Concept,
        eu-aiact:HighRiskAISystem ;
    dct:contributor _:person-delaram-golpayegani,
        _:person-harshvardhan-j-pandit ;
    dct:created "2026-02-09"^^xsd:date ;
    dct:source "AIA(Anx.III)"@en ;
    rdfs:isDefinedBy eu-aiact: ;
    sw:term_status "accepted"@en ;
    skos:broader eu-aiact:HighRiskAISystem-A6-2 ;
    skos:definition "High-risk AI system according to Annex III, Point 4b: Employment, workers management and access to self-employment: AI systems intended to be used to make decisions affecting terms of work-related relationships, the promotion or termination of work-related contractual relationships, to allocate tasks based on individual behaviour or personal traits or characteristics or to monitor and evaluate the performance and behaviour of persons in such relationships"@en ;
    skos:inScheme eu-aiact:highrisk-systems-classes ;
    skos:prefLabel "High-Risk AI System - Annex III(4b)"@en ;
    eu-aiact:hasRiskLevel eu-aiact:RiskLevelHigh-A6-2 .

eu-aiact:HighRiskAISystem-AnnexIII-5-a a rdfs:Class,
        skos:Concept,
        eu-aiact:HighRiskAISystem ;
    dct:contributor _:person-delaram-golpayegani,
        _:person-harshvardhan-j-pandit ;
    dct:created "2026-02-09"^^xsd:date ;
    dct:source "AIA(Anx.III)"@en ;
    rdfs:isDefinedBy eu-aiact: ;
    sw:term_status "accepted"@en ;
    skos:broader eu-aiact:HighRiskAISystem-A6-2 ;
    skos:definition "High-risk AI system according to Annex III, Point 5a: Access to and enjoyment of essential private services and essential public services and benefits: AI systems intended to be used by public authorities or on behalf of public authorities to evaluate the eligibility of natural persons for essential public assistance benefits and services, including healthcare services, as well as to grant, reduce, revoke, or reclaim such benefits and services."@en ;
    skos:inScheme eu-aiact:highrisk-systems-classes ;
    skos:prefLabel "High-Risk AI System - Annex III(5a)"@en ;
    eu-aiact:hasRiskLevel eu-aiact:RiskLevelHigh-A6-2 .

eu-aiact:HighRiskAISystem-AnnexIII-5-b a rdfs:Class,
        skos:Concept,
        eu-aiact:HighRiskAISystem ;
    dct:contributor _:person-delaram-golpayegani,
        _:person-harshvardhan-j-pandit ;
    dct:created "2026-02-09"^^xsd:date ;
    dct:source "AIA(Anx.III)"@en ;
    rdfs:isDefinedBy eu-aiact: ;
    sw:term_status "accepted"@en ;
    skos:broader eu-aiact:HighRiskAISystem-A6-2 ;
    skos:definition "High-risk AI system according to Annex III, Point 5b: Access to and enjoyment of essential private services and essential public services and benefits: AI systems intended to be used to evaluate the creditworthiness of natural persons or establish their credit score, with the exception of AI systems used for the purpose of detecting financial fraud."@en ;
    skos:inScheme eu-aiact:highrisk-systems-classes ;
    skos:prefLabel "High-Risk AI System - Annex III(5b)"@en ;
    eu-aiact:hasRiskLevel eu-aiact:RiskLevelHigh-A6-2 .

eu-aiact:HighRiskAISystem-AnnexIII-5-c a rdfs:Class,
        skos:Concept,
        eu-aiact:HighRiskAISystem ;
    dct:contributor _:person-delaram-golpayegani,
        _:person-harshvardhan-j-pandit ;
    dct:created "2026-02-09"^^xsd:date ;
    dct:source "AIA(Anx.III)"@en ;
    rdfs:isDefinedBy eu-aiact: ;
    sw:term_status "accepted"@en ;
    skos:broader eu-aiact:HighRiskAISystem-A6-2 ;
    skos:definition "High-risk AI system according to Annex III, Point 5c: Access to and enjoyment of essential private services and essential public services and benefits: AI systems intended to be used for risk assessment and pricing in relation to natural persons in the case of life and health insurance."@en ;
    skos:inScheme eu-aiact:highrisk-systems-classes ;
    skos:prefLabel "High-Risk AI System - Annex III(5c)"@en ;
    eu-aiact:hasRiskLevel eu-aiact:RiskLevelHigh-A6-2 .

eu-aiact:HighRiskAISystem-AnnexIII-5-d a rdfs:Class,
        skos:Concept,
        eu-aiact:HighRiskAISystem ;
    dct:contributor _:person-delaram-golpayegani,
        _:person-harshvardhan-j-pandit ;
    dct:created "2026-02-09"^^xsd:date ;
    dct:source "AIA(Anx.III)"@en ;
    rdfs:isDefinedBy eu-aiact: ;
    sw:term_status "accepted"@en ;
    skos:broader eu-aiact:HighRiskAISystem-A6-2 ;
    skos:definition "High-risk AI system according to Annex III, Point 5d: Access to and enjoyment of essential private services and essential public services and benefits: AI systems intended to evaluate and classify emergency calls by natural persons or to be used to dispatch, or to establish priority in the dispatching of, emergency first response services, including by police, firefighters and medical aid, as well as of emergency healthcare patient triage systems."@en ;
    skos:inScheme eu-aiact:highrisk-systems-classes ;
    skos:prefLabel "High-Risk AI System -  Annex III(5d)"@en ;
    eu-aiact:hasRiskLevel eu-aiact:RiskLevelHigh-A6-2 .

eu-aiact:HighRiskAISystem-AnnexIII-6-a a rdfs:Class,
        skos:Concept,
        eu-aiact:HighRiskAISystem ;
    dct:contributor _:person-delaram-golpayegani,
        _:person-harshvardhan-j-pandit ;
    dct:created "2026-02-09"^^xsd:date ;
    dct:source "AIA(Anx.III)"@en ;
    rdfs:isDefinedBy eu-aiact: ;
    sw:term_status "accepted"@en ;
    skos:broader eu-aiact:HighRiskAISystem-A6-2 ;
    skos:definition "High-risk AI system according to Annex III, Point 6a: Law enforcement, in so far as their use is permitted under relevant Union or national law: Law enforcement, in so far as their use is permitted under relevant Union or national law: AI systems intended to be used by or on behalf of law enforcement authorities, or by Union institutions, bodies, offices or agencies in support of law enforcement authorities or on their behalf to assess the risk of a natural person becoming the victim of criminal offences."@en ;
    skos:inScheme eu-aiact:highrisk-systems-classes ;
    skos:prefLabel "High-Risk AI System -  Annex III(6a)"@en ;
    eu-aiact:hasRiskLevel eu-aiact:RiskLevelHigh-A6-2 .

eu-aiact:HighRiskAISystem-AnnexIII-6-b a rdfs:Class,
        skos:Concept,
        eu-aiact:HighRiskAISystem ;
    dct:contributor _:person-delaram-golpayegani,
        _:person-harshvardhan-j-pandit ;
    dct:created "2026-02-09"^^xsd:date ;
    dct:source "AIA(Anx.III)"@en ;
    rdfs:isDefinedBy eu-aiact: ;
    sw:term_status "accepted"@en ;
    skos:broader eu-aiact:HighRiskAISystem-A6-2 ;
    skos:definition "High-risk AI system according to Annex III, Point 6b:  Law enforcement, in so far as their use is permitted under relevant Union or national law: AI systems intended to be used by or on behalf of law enforcement authorities or by Union institutions, bodies, offices or agencies in support of law enforcement authorities as polygraphs or similar tools."@en ;
    skos:inScheme eu-aiact:highrisk-systems-classes ;
    skos:prefLabel "High-Risk AI System -  Annex III(6b)"@en ;
    eu-aiact:hasRiskLevel eu-aiact:RiskLevelHigh-A6-2 .

eu-aiact:HighRiskAISystem-AnnexIII-6-c a rdfs:Class,
        skos:Concept,
        eu-aiact:HighRiskAISystem ;
    dct:contributor _:person-delaram-golpayegani,
        _:person-harshvardhan-j-pandit ;
    dct:created "2026-02-09"^^xsd:date ;
    dct:source "AIA(Anx.III)"@en ;
    rdfs:isDefinedBy eu-aiact: ;
    sw:term_status "accepted"@en ;
    skos:broader eu-aiact:HighRiskAISystem-A6-2 ;
    skos:definition "High-risk AI system according to Annex III, Point 6c:  AI systems intended to be used by or on behalf of law enforcement authorities, or by Union institutions, bodies, offices or agencies, in support of law enforcement authorities to evaluate the reliability of evidence in the course of the investigation or prosecution of criminal offences."@en ;
    skos:inScheme eu-aiact:highrisk-systems-classes ;
    skos:prefLabel "High-Risk AI System -  Annex III(6c)"@en ;
    eu-aiact:hasRiskLevel eu-aiact:RiskLevelHigh-A6-2 .

eu-aiact:HighRiskAISystem-AnnexIII-6-d a rdfs:Class,
        skos:Concept,
        eu-aiact:HighRiskAISystem ;
    dct:contributor _:person-delaram-golpayegani,
        _:person-harshvardhan-j-pandit ;
    dct:created "2026-02-09"^^xsd:date ;
    dct:source "AIA(Anx.III)"@en ;
    rdfs:isDefinedBy eu-aiact: ;
    sw:term_status "accepted"@en ;
    skos:broader eu-aiact:HighRiskAISystem-A6-2 ;
    skos:definition "High-risk AI system according to Annex III, Point 6d:  Law enforcement, in so far as their use is permitted under relevant Union or national law: AI systems intended to be used by law enforcement authorities or on their behalf or by Union institutions, bodies, offices or agencies in support of law enforcement authorities for assessing the risk of a natural person offending or re-offending not solely on the basis of the profiling of natural persons as referred to in Article 3(4) of Directive (EU) 2016/680, or to assess personality traits and characteristics or past criminal behaviour of natural persons or groups."@en ;
    skos:inScheme eu-aiact:highrisk-systems-classes ;
    skos:prefLabel "High-Risk AI System -  Annex III(6d)"@en ;
    eu-aiact:hasRiskLevel eu-aiact:RiskLevelHigh-A6-2 .

eu-aiact:HighRiskAISystem-AnnexIII-6-e a rdfs:Class,
        skos:Concept,
        eu-aiact:HighRiskAISystem ;
    dct:contributor _:person-delaram-golpayegani,
        _:person-harshvardhan-j-pandit ;
    dct:created "2026-02-09"^^xsd:date ;
    dct:source "AIA(Anx.III)"@en ;
    rdfs:isDefinedBy eu-aiact: ;
    sw:term_status "accepted"@en ;
    skos:broader eu-aiact:HighRiskAISystem-A6-2 ;
    skos:definition "High-risk AI system according to Annex III, Point 6e:  Law enforcement, in so far as their use is permitted under relevant Union or national law: AI systems intended to be used by or on behalf of law enforcement authorities or by Union institutions, bodies, offices or agencies in support of law enforcement authorities for the profiling of natural persons as referred to in Article 3(4) of Directive (EU) 2016/680 in the course of the detection, investigation or prosecution of criminal offences."@en ;
    skos:inScheme eu-aiact:highrisk-systems-classes ;
    skos:prefLabel "High-Risk AI System -  Annex III(6e)"@en ;
    eu-aiact:hasRiskLevel eu-aiact:RiskLevelHigh-A6-2 .

eu-aiact:HighRiskAISystem-AnnexIII-7-a a rdfs:Class,
        skos:Concept,
        eu-aiact:HighRiskAISystem ;
    dct:contributor _:person-delaram-golpayegani,
        _:person-harshvardhan-j-pandit ;
    dct:created "2026-02-09"^^xsd:date ;
    dct:source "AIA(Anx.III)"@en ;
    rdfs:isDefinedBy eu-aiact: ;
    sw:term_status "accepted"@en ;
    skos:broader eu-aiact:HighRiskAISystem-A6-2 ;
    skos:definition "High-risk AI system according to Annex III, Point 7a: Migration, asylum and border control management, in so far as their use is permitted under relevant Union or national law: AI systems intended to be used by or on behalf of competent public authorities or by Union institutions, bodies, offices or agencies as polygraphs or similar tools."@en ;
    skos:inScheme eu-aiact:highrisk-systems-classes ;
    skos:prefLabel "High-Risk AI System -  Annex III(7a)"@en ;
    eu-aiact:hasRiskLevel eu-aiact:RiskLevelHigh-A6-2 .

eu-aiact:HighRiskAISystem-AnnexIII-7-b a rdfs:Class,
        skos:Concept,
        eu-aiact:HighRiskAISystem ;
    dct:contributor _:person-delaram-golpayegani,
        _:person-harshvardhan-j-pandit ;
    dct:created "2026-02-09"^^xsd:date ;
    dct:source "AIA(Anx.III)"@en ;
    rdfs:isDefinedBy eu-aiact: ;
    sw:term_status "accepted"@en ;
    skos:broader eu-aiact:HighRiskAISystem-A6-2 ;
    skos:definition "High-risk AI system according to Annex III, Point 7b: Migration, asylum and border control management, in so far as their use is permitted under relevant Union or national law: AI systems intended to be used by or on behalf of competent public authorities or by Union institutions, bodies, offices or agencies to assess a risk, including a security risk, a risk of irregular migration, or a health risk, posed by a natural person who intends to enter or who has entered into the territory of a Member State."@en ;
    skos:inScheme eu-aiact:highrisk-systems-classes ;
    skos:prefLabel "High-Risk AI System -  Annex III(7b)"@en ;
    eu-aiact:hasRiskLevel eu-aiact:RiskLevelHigh-A6-2 .

eu-aiact:HighRiskAISystem-AnnexIII-7-c a rdfs:Class,
        skos:Concept,
        eu-aiact:HighRiskAISystem ;
    dct:contributor _:person-delaram-golpayegani,
        _:person-harshvardhan-j-pandit ;
    dct:created "2026-02-09"^^xsd:date ;
    dct:source "AIA(Anx.III)"@en ;
    rdfs:isDefinedBy eu-aiact: ;
    sw:term_status "accepted"@en ;
    skos:broader eu-aiact:HighRiskAISystem-A6-2 ;
    skos:definition "High-risk AI system according to Annex III, Point 7c: Migration, asylum and border control management, in so far as their use is permitted under relevant Union or national law: AI systems intended to be used by or on behalf of competent public authorities or by Union institutions, bodies, offices or agencies to assist competent public authorities for the examination of applications for asylum, visa or residence permits and for associated complaints with regard to the eligibility of the natural persons applying for a status, including related assessments of the reliability of evidence."@en ;
    skos:inScheme eu-aiact:highrisk-systems-classes ;
    skos:prefLabel "High-Risk AI System -  Annex III(7c)"@en ;
    eu-aiact:hasRiskLevel eu-aiact:RiskLevelHigh-A6-2 .

eu-aiact:HighRiskAISystem-AnnexIII-7-d a rdfs:Class,
        skos:Concept,
        eu-aiact:HighRiskAISystem ;
    dct:contributor _:person-delaram-golpayegani,
        _:person-harshvardhan-j-pandit ;
    dct:created "2026-02-09"^^xsd:date ;
    dct:source "AIA(Anx.III)"@en ;
    rdfs:isDefinedBy eu-aiact: ;
    sw:term_status "accepted"@en ;
    skos:broader eu-aiact:HighRiskAISystem-A6-2 ;
    skos:definition "High-risk AI system according to Annex III, Point 7d: Migration, asylum and border control management, in so far as their use is permitted under relevant Union or national law: AI systems intended to be used by or on behalf of competent public authorities, or by Union institutions, bodies, offices or agencies, in the context of migration, asylum or border control management, for the purpose of detecting, recognising or identifying natural persons, with the exception of the verification of travel documents."@en ;
    skos:inScheme eu-aiact:highrisk-systems-classes ;
    skos:prefLabel "High-Risk AI System -  Annex III(7d)"@en ;
    eu-aiact:hasRiskLevel eu-aiact:RiskLevelHigh-A6-2 .

eu-aiact:HighRiskAISystem-AnnexIII-8-a a rdfs:Class,
        skos:Concept,
        eu-aiact:HighRiskAISystem ;
    dct:contributor _:person-delaram-golpayegani,
        _:person-harshvardhan-j-pandit ;
    dct:created "2026-02-09"^^xsd:date ;
    dct:source "AIA(Anx.III)"@en ;
    rdfs:isDefinedBy eu-aiact: ;
    sw:term_status "accepted"@en ;
    skos:broader eu-aiact:HighRiskAISystem-A6-2 ;
    skos:definition "High-risk AI system according to Annex III, Point 8a: Administration of justice and democratic processes: AI systems intended to be used by a judicial authority or on their behalf to assist a judicial authority in researching and interpreting facts and the law and in applying the law to a concrete set of facts, or to be used in a similar way in alternative dispute resolution."@en ;
    skos:inScheme eu-aiact:highrisk-systems-classes ;
    skos:prefLabel "High-Risk AI System -  Annex III(8a)"@en ;
    eu-aiact:hasRiskLevel eu-aiact:RiskLevelHigh-A6-2 .

eu-aiact:HighRiskAISystem-AnnexIII-8-b a rdfs:Class,
        skos:Concept,
        eu-aiact:HighRiskAISystem ;
    dct:contributor _:person-delaram-golpayegani,
        _:person-harshvardhan-j-pandit ;
    dct:created "2026-02-09"^^xsd:date ;
    dct:source "AIA(Anx.III)"@en ;
    rdfs:isDefinedBy eu-aiact: ;
    sw:term_status "accepted"@en ;
    skos:broader eu-aiact:HighRiskAISystem-A6-2 ;
    skos:definition "High-risk AI system according to Annex III, Point 8b: Administration of justice and democratic processes: AI systems intended to be used for influencing the outcome of an election or referendum or the voting behaviour of natural persons in the exercise of their vote in elections or referenda. This does not include AI systems to the output of which natural persons are not directly exposed, such as tools used to organise, optimise or structure political campaigns from an administrative or logistical point of view."@en ;
    skos:inScheme eu-aiact:highrisk-systems-classes ;
    skos:prefLabel "High-Risk AI System -  Annex III(8b)"@en ;
    eu-aiact:hasRiskLevel eu-aiact:RiskLevelHigh-A6-2 .

eu-aiact:HumanOverseer a rdfs:Class,
        skos:Concept ;
    dct:contributor _:person-delaram-golpayegani,
        _:person-harshvardhan-j-pandit ;
    dct:created "2026-02-09"^^xsd:date ;
    rdfs:isDefinedBy eu-aiact: ;
    rdfs:subClassOf dpv:NaturalPerson,
        tech:Actor ;
    sw:term_status "accepted"@en ;
    skos:broader dpv:NaturalPerson,
        tech:Actor ;
    skos:definition "The natural person to whom human oversight is assigned"@en ;
    skos:inScheme eu-aiact:roles-classes ;
    skos:prefLabel "Human Overseer"@en .

eu-aiact:InformedConsent a rdfs:Class,
        skos:Concept,
        dpv:LegalBasis ;
    dct:contributor _:person-delaram-golpayegani ;
    dct:created "2024-04-10"^^xsd:date ;
    dct:modified "2024-07-30"^^xsd:date ;
    dct:source "AIA (Art. 3(59))"@en ;
    rdfs:isDefinedBy eu-aiact: ;
    sw:term_status "modified"@en ;
    skos:broader dpv:InformedConsent ;
    skos:definition "Informed consent means a (real world test) subject’s freely given, specific, unambiguous and voluntary expression of his or her willingness to participate in a particular testing in real world conditions, after having been informed of all aspects of the testing that are relevant to the subject’s decision to participate"@en ;
    skos:inScheme eu-aiact:assessment-classes ;
    skos:prefLabel "Informed Consent"@en .

eu-aiact:InstructionForUse a rdfs:Class,
        skos:Concept,
        tech:Documentation ;
    dct:contributor _:person-delaram-golpayegani ;
    dct:created "2024-04-10"^^xsd:date ;
    dct:modified "2025-07-31"^^xsd:date ;
    dct:source "AIA(Art.3(15))"@en ;
    rdfs:isDefinedBy eu-aiact: ;
    sw:term_status "modified"@en ;
    skos:broader tech:Instructions ;
    skos:definition "The information provided by the provider to inform the deployer of, in particular, an AI system’s intended purpose and proper use"@en ;
    skos:inScheme eu-aiact:docs-classes ;
    skos:prefLabel "Instruction For Use"@en .

eu-aiact:IntendedPurpose a rdfs:Class,
        skos:Concept ;
    dct:contributor _:person-delaram-golpayegani ;
    dct:created "2024-04-10"^^xsd:date ;
    dct:source "AIA (Art. 3(12))"@en ;
    rdfs:isDefinedBy eu-aiact: ;
    rdfs:subClassOf tech:IntendedUse ;
    sw:term_status "accepted"@en ;
    skos:broader tech:IntendedUse ;
    skos:definition "The use for which an AI system is intended by the provider, including the specific context and conditions of use, as specified in the information supplied by the provider in the instructions for use, promotional or sales materials and statements, as well as in the technical documentation"@en ;
    skos:inScheme eu-aiact:misc-classes ;
    skos:prefLabel "Intended Purpose"@en .

eu-aiact:JusticeSector a rdfs:Class,
        skos:Concept,
        dpv:Sector ;
    dct:contributor _:person-delaram-golpayegani,
        _:person-harshvardhan-j-pandit ;
    dct:created "2024-12-01"^^xsd:date ;
    dct:source " Annex III"@en,
        "EU AI Act"@en ;
    rdfs:isDefinedBy eu-aiact: ;
    sw:term_status "accepted"@en ;
    skos:broader dpv:Sector ;
    skos:definition "Sector related to administration of justice"@en ;
    skos:inScheme eu-aiact:sector-classes ;
    skos:prefLabel "Justice Sector"@en .

eu-aiact:LawEnforcementSector a rdfs:Class,
        skos:Concept,
        dpv:Sector ;
    dct:contributor _:person-delaram-golpayegani,
        _:person-harshvardhan-j-pandit ;
    dct:created "2024-12-01"^^xsd:date ;
    dct:source " Annex III"@en,
        "EU AI Act"@en ;
    rdfs:isDefinedBy eu-aiact: ;
    sw:term_status "accepted"@en ;
    skos:broader dpv:Sector ;
    skos:definition "Sector related to law enforcement"@en ;
    skos:inScheme eu-aiact:sector-classes ;
    skos:prefLabel "Law Enforcement Sector"@en .

eu-aiact:MarketAvailabilityStatus a rdfs:Class,
        skos:Concept ;
    dct:contributor _:person-delaram-golpayegani ;
    dct:created "2024-05-17"^^xsd:date ;
    rdfs:isDefinedBy eu-aiact: ;
    rdfs:subClassOf tech:MarketAvailabilityStatus ;
    sw:term_status "accepted"@en ;
    skos:broader tech:MarketAvailabilityStatus ;
    skos:definition "Status associated with whether the AI system or GPAI Model is available for distribution or use on the market in the course of a commercial activity"@en ;
    skos:inScheme eu-aiact:status-classes ;
    skos:prefLabel "Market Availability Status"@en .

eu-aiact:MarketPlacementStatus a rdfs:Class,
        skos:Concept ;
    dct:contributor _:person-delaram-golpayegani ;
    dct:created "2024-05-17"^^xsd:date ;
    rdfs:isDefinedBy eu-aiact: ;
    rdfs:subClassOf tech:MarketAvailabilityStatus ;
    sw:term_status "accepted"@en ;
    skos:broader tech:MarketAvailabilityStatus ;
    skos:definition "Status associated with whether the AI system or GPAI Model has been 'first' made available on the market"@en ;
    skos:inScheme eu-aiact:status-classes ;
    skos:prefLabel "Market Placement Status"@en .

eu-aiact:MarketSurveillanceAuthority a rdfs:Class,
        skos:Concept ;
    dct:contributor _:person-delaram-golpayegani ;
    dct:created "2024-04-10"^^xsd:date ;
    dct:source "AIA(Art. 3(26))"@en ;
    rdfs:isDefinedBy eu-aiact: ;
    rdfs:subClassOf eu-aiact:NationalCompetentAuthority ;
    sw:term_status "accepted"@en ;
    skos:broader eu-aiact:NationalCompetentAuthority ;
    skos:definition "The national authority carrying out the activities and taking the measures pursuant to Regulation (EU) 2019/1020"@en ;
    skos:inScheme eu-aiact:roles-classes ;
    skos:prefLabel "Market Surveillance Authority"@en .

eu-aiact:MigrationSector a rdfs:Class,
        skos:Concept,
        dpv:Sector ;
    dct:contributor _:person-delaram-golpayegani,
        _:person-harshvardhan-j-pandit ;
    dct:created "2024-12-01"^^xsd:date ;
    dct:source " Annex III"@en,
        "EU AI Act"@en ;
    rdfs:isDefinedBy eu-aiact: ;
    sw:term_status "accepted"@en ;
    skos:broader dpv:Sector ;
    skos:definition "Sector related to migration management"@en ;
    skos:inScheme eu-aiact:sector-classes ;
    skos:prefLabel "Migration Sector"@en .

eu-aiact:NationalCompetentAuthority a rdfs:Class,
        skos:Concept ;
    dct:contributor _:person-delaram-golpayegani ;
    dct:created "2024-04-10"^^xsd:date ;
    dct:modified "2027-07-30"^^xsd:date ;
    dct:source "AIA(Art. 3(48))"@en ;
    rdfs:isDefinedBy eu-aiact: ;
    rdfs:subClassOf dpv:Authority ;
    sw:term_status "modified"@en ;
    skos:broader dpv:Authority ;
    skos:definition "A notifying authority or a market surveillance authority; as regards AI systems put into service or used by Union institutions, agencies, offices and bodies, references to national competent authorities or market surveillance authorities in the AI Act shall be construed as references to the European Data Protection Supervisor"@en ;
    skos:inScheme eu-aiact:roles-classes ;
    skos:prefLabel "National Competent Authority"@en .

eu-aiact:NonpredeterminedChange a rdfs:Class,
        skos:Concept,
        eu-aiact:ChangeCategory ;
    dct:contributor _:person-delaram-golpayegani ;
    dct:created "2024-12-01"^^xsd:date ;
    rdfs:isDefinedBy eu-aiact: ;
    sw:term_status "accepted"@en ;
    skos:broader eu-aiact:ChangeCategory ;
    skos:definition "Change associated with the AI system that has not been pre-determined"@en ;
    skos:inScheme eu-aiact:status-classes ;
    skos:prefLabel "Non-Predetermined Change"@en ;
    skos:scopeNote "What is considered \"pre-determined\" is not defined with this concept or within the AI Act, therefore if there are specific interpretations of \"pre-determined\", such as within a jurisdiction, sector, or for a particular technology, then this concept should be extended accordingly"@en .

eu-aiact:NotAvailableOnMarket a rdfs:Class,
        skos:Concept,
        eu-aiact:MarketAvailabilityStatus ;
    dct:contributor _:person-delaram-golpayegani ;
    dct:created "2024-05-17"^^xsd:date ;
    rdfs:isDefinedBy eu-aiact: ;
    sw:term_status "accepted"@en ;
    skos:broader eu-aiact:MarketAvailabilityStatus ;
    skos:definition "not available on a market anywhere in EU or otherwise"@en ;
    skos:inScheme eu-aiact:status-classes ;
    skos:prefLabel "Not Available on Market"@en .

eu-aiact:NotPutIntoService a rdfs:Class,
        skos:Concept,
        eu-aiact:ServiceSupplyStatus ;
    dct:contributor _:person-delaram-golpayegani ;
    dct:created "2024-05-17"^^xsd:date ;
    rdfs:isDefinedBy eu-aiact: ;
    sw:term_status "accepted"@en ;
    skos:broader eu-aiact:ServiceSupplyStatus ;
    skos:definition "Status associated with an AI system that has not been put into service"@en ;
    skos:inScheme eu-aiact:status-classes ;
    skos:prefLabel "Not Put in to Service"@en .

eu-aiact:NotifiedBody a rdfs:Class,
        skos:Concept ;
    dct:contributor _:person-delaram-golpayegani ;
    dct:created "2024-04-10"^^xsd:date ;
    dct:source "AIA(Art. 3(22))"@en ;
    rdfs:isDefinedBy eu-aiact: ;
    rdfs:subClassOf eu-aiact:ConformityAssessmentBody ;
    sw:term_status "accepted"@en ;
    skos:broader eu-aiact:ConformityAssessmentBody ;
    skos:definition "A conformity assessment body notified in accordance with the AI Act and other relevant Union harmonisation legislation"@en ;
    skos:inScheme eu-aiact:roles-classes ;
    skos:prefLabel "Notified Body"@en .

eu-aiact:NotifyingAuthority a rdfs:Class,
        skos:Concept ;
    dct:contributor _:person-delaram-golpayegani ;
    dct:created "2024-04-10"^^xsd:date ;
    dct:source "AIA(Art. 3(19))"@en ;
    rdfs:isDefinedBy eu-aiact: ;
    rdfs:subClassOf eu-aiact:NationalCompetentAuthority ;
    sw:term_status "accepted"@en ;
    skos:broader eu-aiact:NationalCompetentAuthority ;
    skos:definition "The national authority responsible for setting up and carrying out the necessary procedures for the assessment, designation and notification of conformity assessment bodies and for their monitoring"@en ;
    skos:inScheme eu-aiact:roles-classes ;
    skos:prefLabel "Notifying Authority"@en .

eu-aiact:PlacedOnEUMarket a rdfs:Class,
        skos:Concept,
        eu-aiact:MarketPlacementStatus ;
    dct:contributor _:person-delaram-golpayegani ;
    dct:created "2024-05-17"^^xsd:date ;
    dct:source "AIA (Art. 3(9))"@en ;
    rdfs:isDefinedBy eu-aiact: ;
    sw:term_status "accepted"@en ;
    skos:broader eu-aiact:PlacedOnMarket ;
    skos:definition "Status indicating the first making available of an AI system or a general purpose AI model on the Union market"@en ;
    skos:inScheme eu-aiact:status-classes ;
    skos:prefLabel "Placed on EU Market"@en .

eu-aiact:PlacedOnMarket a rdfs:Class,
        skos:Concept,
        eu-aiact:MarketPlacementStatus ;
    dct:contributor _:person-delaram-golpayegani ;
    dct:created "2024-05-17"^^xsd:date ;
    dct:source "AIA (Art. 3(9))"@en ;
    rdfs:isDefinedBy eu-aiact: ;
    sw:term_status "accepted"@en ;
    skos:broader eu-aiact:MarketPlacementStatus ;
    skos:definition "Status indicating the first making available of an AI system or a general purpose AI model on the market"@en ;
    skos:inScheme eu-aiact:status-classes ;
    skos:prefLabel "Placed on Market"@en .

eu-aiact:PostMarketMonitoringPlan a rdfs:Class,
        skos:Concept,
        tech:Documentation ;
    dct:contributor _:person-delaram-golpayegani ;
    dct:created "2024-12-01"^^xsd:date ;
    dct:modified "2024-12-17"^^xsd:date ;
    dct:source "AI Act Art.72"@en ;
    rdfs:isDefinedBy eu-aiact: ;
    sw:term_status "modified"@en ;
    skos:broader tech:Plan ;
    skos:definition "Description of the post-market monitoring plan, as required by the AI Act"@en ;
    skos:inScheme eu-aiact:docs-classes ;
    skos:prefLabel "Post-market Monitoring Plan"@en .

eu-aiact:PostMarketMonitoringSystem a rdfs:Class,
        skos:Concept,
        dpv:OrganisationalMeasure ;
    dct:contributor _:person-delaram-golpayegani ;
    dct:created "2024-04-10"^^xsd:date ;
    dct:source "AIA(Art. 3(25))"@en ;
    rdfs:isDefinedBy eu-aiact: ;
    sw:term_status "accepted"@en ;
    skos:broader dpv:OrganisationalMeasure ;
    skos:definition """All activities carried out by providers of AI systems to collect and review experience gained from the use of AI systems they
place on the market or put into service for the purpose of identifying any need to immediately apply any necessary corrective or preventive actions"""@en ;
    skos:inScheme eu-aiact:assessment-classes ;
    skos:prefLabel "Post-Market Monitoring System"@en .

eu-aiact:PostMarketMonitoringSystemDocumentation a rdfs:Class,
        skos:Concept,
        tech:Documentation ;
    dct:contributor _:person-delaram-golpayegani ;
    dct:created "2024-12-01"^^xsd:date ;
    dct:source "AI Act Art.72"@en ;
    rdfs:isDefinedBy eu-aiact: ;
    sw:term_status "accepted"@en ;
    skos:broader tech:Documentation ;
    skos:definition "Documentation of the post-market monitoring system in place, as required by the AI Act"@en ;
    skos:inScheme eu-aiact:docs-classes ;
    skos:prefLabel "Post-market Monitoring System Documentation"@en .

eu-aiact:PostRemoteBiometricIdentificationSystem a rdfs:Class,
        skos:Concept,
        eu-aiact:AISystem ;
    dct:contributor _:person-delaram-golpayegani ;
    dct:created "2024-04-10"^^xsd:date ;
    dct:modified "2025-07-30"^^xsd:date ;
    dct:source "AIA(Art. 3(43))"@en ;
    rdfs:isDefinedBy eu-aiact: ;
    sw:term_status "modified"@en ;
    skos:broader eu-aiact:RemoteBiometricIdentificationSystem ;
    skos:definition "A remote biometric identification system other than a real-time remote biometric identification system"@en ;
    skos:inScheme eu-aiact:system-classes ;
    skos:prefLabel "Post Remote Biometric Identification System"@en ;
    skos:related pd:Biometric .

eu-aiact:PredeterminedChange a rdfs:Class,
        skos:Concept,
        eu-aiact:ChangeCategory ;
    dct:contributor _:person-delaram-golpayegani ;
    dct:created "2024-12-01"^^xsd:date ;
    rdfs:isDefinedBy eu-aiact: ;
    sw:term_status "accepted"@en ;
    skos:broader eu-aiact:ChangeCategory ;
    skos:definition "Change associated with the AI system that has been pre-determined"@en ;
    skos:inScheme eu-aiact:status-classes ;
    skos:prefLabel "Predetermined Change"@en ;
    skos:scopeNote "What is considered \"pre-determined\" is not defined with this concept or within the AI Act, therefore if there are specific interpretations of \"pre-determined\", such as within a jurisdiction, sector, or for a particular technology, then this concept should be extended accordingly"@en .

eu-aiact:PrivateSector a rdfs:Class,
        skos:Concept,
        dpv:Sector ;
    dct:contributor _:person-delaram-golpayegani,
        _:person-harshvardhan-j-pandit ;
    dct:created "2024-12-01"^^xsd:date ;
    dct:source " Annex III"@en,
        "EU AI Act"@en ;
    rdfs:isDefinedBy eu-aiact: ;
    sw:term_status "accepted"@en ;
    skos:broader dpv:Sector ;
    skos:definition "Sector comprising of entities that are privately owned"@en ;
    skos:inScheme eu-aiact:sector-classes ;
    skos:prefLabel "Private Sector"@en .

eu-aiact:ProhibitedAISystem a rdfs:Class,
        skos:Concept ;
    dct:contributor _:person-delaram-golpayegani,
        _:person-harshvardhan-j-pandit ;
    dct:created "2026-02-09"^^xsd:date ;
    dct:source "AIA(Art.5)"@en ;
    rdfs:isDefinedBy eu-aiact: ;
    rdfs:subClassOf eu-aiact:AISystem ;
    sw:term_status "accepted"@en ;
    skos:broader eu-aiact:AISystem ;
    skos:definition "Prohibited AI system according to Article 5, AI Act"@en ;
    skos:inScheme eu-aiact:system-classes ;
    skos:prefLabel "Prohibited AI System"@en .

eu-aiact:ProhibitedAISystem-A5-1-a a rdfs:Class,
        skos:Concept,
        eu-aiact:ProhibitedAISystem ;
    dct:contributor _:person-delaram-golpayegani ;
    dct:created "2026-02-09"^^xsd:date ;
    dct:source "AIA(Art.5(1a))"@en ;
    rdfs:isDefinedBy eu-aiact: ;
    sw:term_status "accepted"@en ;
    skos:broader eu-aiact:ProhibitedAISystem ;
    skos:definition "Prohibited AI system according to Article 5(1a) of the AI Act, indicating an AI system that deploys subliminal techniques beyond a person’s consciousness or purposefully manipulative or deceptive techniques, with the objective, or the effect of materially distorting the behaviour of a person or a group of persons by appreciably impairing their ability to make an informed decision, thereby causing them to take a decision that they would not have otherwise taken in a manner that causes or is reasonably likely to cause that person, another person or group of persons significant harm."@en ;
    skos:inScheme eu-aiact:prohibited-systems-classes ;
    skos:prefLabel "Prohibited AI System - Article 5(1a)"@en ;
    eu-aiact:hasRiskLevel eu-aiact:RiskLevelProhibited .

eu-aiact:ProhibitedAISystem-A5-1-b a rdfs:Class,
        skos:Concept,
        eu-aiact:ProhibitedAISystem ;
    dct:contributor _:person-delaram-golpayegani ;
    dct:created "2026-02-09"^^xsd:date ;
    dct:source "AIA(Art.5(1b))"@en ;
    rdfs:isDefinedBy eu-aiact: ;
    sw:term_status "accepted"@en ;
    skos:broader eu-aiact:ProhibitedAISystem ;
    skos:definition "Prohibited AI system according to Article 5(1b) of the AI Act, indicating an AI system that exploits any of the vulnerabilities of a natural person or a specific group of persons due to their age, disability or a specific social or economic situation, with the objective, or the effect, of materially distorting the behaviour of that person or a person belonging to that group in a manner that causes or is reasonably likely to cause that person or another person significant harm."@en ;
    skos:inScheme eu-aiact:prohibited-systems-classes ;
    skos:prefLabel "Prohibited AI System - Article 5(1b)"@en ;
    eu-aiact:hasRiskLevel eu-aiact:RiskLevelProhibited .

eu-aiact:ProhibitedAISystem-A5-1-c a rdfs:Class,
        skos:Concept,
        eu-aiact:ProhibitedAISystem ;
    dct:contributor _:person-delaram-golpayegani ;
    dct:created "2026-02-09"^^xsd:date ;
    dct:source "AIA(Art.5(1c))"@en ;
    rdfs:isDefinedBy eu-aiact: ;
    sw:term_status "accepted"@en ;
    skos:broader eu-aiact:ProhibitedAISystem ;
    skos:definition "Prohibited AI system according to Article 5(1c) of the AI Act, indicating AI systems that evaluate or classify of natural persons or groups of persons over a certain period of time based on their social behaviour or known, inferred or predicted personal or personality characteristics, with the social score leading to either or both of the following:  (i) detrimental or unfavourable treatment of certain natural persons or groups of persons in social contexts that are unrelated to the contexts in which the data was originally generated or collected; (ii) detrimental or unfavourable treatment of certain natural persons or groups of persons that is unjustified or disproportionate to their social behaviour or its gravity;"@en ;
    skos:inScheme eu-aiact:prohibited-systems-classes ;
    skos:prefLabel "Prohibited AI System - Article 5(1c)"@en ;
    eu-aiact:hasRiskLevel eu-aiact:RiskLevelProhibited .

eu-aiact:ProhibitedAISystem-A5-1-d a rdfs:Class,
        skos:Concept,
        eu-aiact:ProhibitedAISystem ;
    dct:contributor _:person-delaram-golpayegani ;
    dct:created "2026-02-09"^^xsd:date ;
    dct:source "AIA(Art.5(1d))"@en ;
    rdfs:isDefinedBy eu-aiact: ;
    sw:term_status "accepted"@en ;
    skos:broader eu-aiact:ProhibitedAISystem ;
    skos:definition "Prohibited AI system according to Article 5(1d) of the AI Act, indicating AI system used for making risk assessments of natural persons in order to assess or predict the risk of a natural person committing a criminal offence, based solely on the profiling of a natural person or on assessing their personality traits and characteristics; this prohibition shall not apply to AI systems used to support the human assessment of the involvement of a person in a criminal activity, which is already based on objective and verifiable facts directly linked to a criminal activity"@en ;
    skos:inScheme eu-aiact:prohibited-systems-classes ;
    skos:prefLabel "Prohibited AI System -  Article 5(1d)"@en ;
    eu-aiact:hasRiskLevel eu-aiact:RiskLevelProhibited .

eu-aiact:ProhibitedAISystem-A5-1-e a rdfs:Class,
        skos:Concept,
        eu-aiact:ProhibitedAISystem ;
    dct:contributor _:person-delaram-golpayegani ;
    dct:created "2026-02-09"^^xsd:date ;
    dct:source "AIA(Art.5(1e))"@en ;
    rdfs:isDefinedBy eu-aiact: ;
    sw:term_status "accepted"@en ;
    skos:broader eu-aiact:ProhibitedAISystem ;
    skos:definition "Prohibited AI system according to Article 5(1e) of the AI Act, indicating AI systems that create or expand facial recognition databases through the untargeted scraping of facial images from the internet or CCTV footage"@en ;
    skos:inScheme eu-aiact:prohibited-systems-classes ;
    skos:prefLabel "Prohibited AI System - Article 5(1e)"@en ;
    eu-aiact:hasRiskLevel eu-aiact:RiskLevelProhibited .

eu-aiact:ProhibitedAISystem-A5-1-f a rdfs:Class,
        skos:Concept,
        eu-aiact:ProhibitedAISystem ;
    dct:contributor _:person-delaram-golpayegani ;
    dct:created "2026-02-09"^^xsd:date ;
    dct:source "AIA(Art.5(1f))"@en ;
    rdfs:isDefinedBy eu-aiact: ;
    sw:term_status "accepted"@en ;
    skos:broader eu-aiact:ProhibitedAISystem ;
    skos:definition """Prohibited AI system according to Article 5(1f) of the AI Act, indicating  AI systems that infer emotions of a natural person in the areas of workplace and education institutions, except where the use of the AI system is
intended to be put in place or into the market for medical or safety reasons"""@en ;
    skos:inScheme eu-aiact:prohibited-systems-classes ;
    skos:prefLabel "Prohibited AI System - Article 5(1f)"@en ;
    eu-aiact:hasRiskLevel eu-aiact:RiskLevelProhibited .

eu-aiact:ProhibitedAISystem-A5-1-g a rdfs:Class,
        skos:Concept,
        eu-aiact:ProhibitedAISystem ;
    dct:contributor _:person-delaram-golpayegani ;
    dct:created "2026-02-09"^^xsd:date ;
    dct:source "AIA(Art.5(1g))"@en ;
    rdfs:isDefinedBy eu-aiact: ;
    sw:term_status "accepted"@en ;
    skos:broader eu-aiact:ProhibitedAISystem ;
    skos:definition """Prohibited AI system / risk level according to Article 5(1g) of the AI Act, indicating biometric categorisation systems that categorise individually natural persons based on their biometric data to deduce or infer their race, political
opinions, trade union membership, religious or philosophical beliefs, sex life or sexual orientation; this prohibition does
not cover any labelling or filtering of lawfully acquired biometric datasets, such as images, based on biometric data or
categorizing of biometric data in the area of law enforcement."""@en ;
    skos:inScheme eu-aiact:prohibited-systems-classes ;
    skos:prefLabel "Prohibited AI System - Article 5(1g)"@en ;
    eu-aiact:hasRiskLevel eu-aiact:RiskLevelProhibited .

eu-aiact:ProhibitedAISystem-A5-1-h a rdfs:Class,
        skos:Concept,
        eu-aiact:ProhibitedAISystem ;
    dct:contributor _:person-delaram-golpayegani ;
    dct:created "2026-02-09"^^xsd:date ;
    dct:source "AIA(Art.5(1h))"@en ;
    rdfs:isDefinedBy eu-aiact: ;
    sw:term_status "accepted"@en ;
    skos:broader eu-aiact:ProhibitedAISystem ;
    skos:definition """Prohibited AI system according to Article 5(1h) of the AI Act,  the use of ‘real-time’ remote biometric identification systems in publicly accessible spaces for the purposes of law enforcement, unless and in so far as such use is strictly necessary for one of the following objectives:
(i) the targeted search for specific victims of abduction, trafficking in human beings or sexual exploitation of human
beings, as well as the search for missing persons;
(ii) the prevention of a specific, substantial and imminent threat to the life or physical safety of natural persons or
a genuine and present or genuine and foreseeable threat of a terrorist attack;
(iii) the localisation or identification of a person suspected of having committed a criminal offence, for the purpose of
conducting a criminal investigation or prosecution or executing a criminal penalty for offences referred to in
Annex II and punishable in the Member State concerned by a custodial sentence or a detention order for
a maximum period of at least four years."""@en ;
    skos:inScheme eu-aiact:prohibited-systems-classes ;
    skos:prefLabel "Prohibited AI System - Article 5(1h)"@en ;
    eu-aiact:hasRiskLevel eu-aiact:RiskLevelProhibited .

eu-aiact:ProviderHumanOversightMeasure a rdfs:Class,
        skos:Concept,
        dpv:OrganisationalMeasure ;
    dct:contributor _:person-delaram-golpayegani,
        _:person-harshvardhan-j-pandit ;
    dct:created "2026-02-09"^^xsd:date ;
    dct:source " Art. 14 (3a)"@en,
        "AI Act"@en ;
    rdfs:isDefinedBy eu-aiact: ;
    sw:term_status "accepted"@en ;
    skos:broader dpv:HumanOversight ;
    skos:definition "Human oversight measures built into the AI system by the provider before it is placed on the market or put into service."@en ;
    skos:inScheme eu-aiact:risk-classes ;
    skos:prefLabel "Human Oversight Measure by Provider"@en .

eu-aiact:PublicSector a rdfs:Class,
        skos:Concept,
        dpv:Sector ;
    dct:contributor _:person-delaram-golpayegani,
        _:person-harshvardhan-j-pandit ;
    dct:created "2024-12-01"^^xsd:date ;
    dct:source " Annex III"@en,
        "EU AI Act"@en ;
    rdfs:isDefinedBy eu-aiact: ;
    sw:term_status "accepted"@en ;
    skos:broader dpv:Sector ;
    skos:definition "Sector comprising of entities that are publicly owned e.g. by the government"@en ;
    skos:inScheme eu-aiact:sector-classes ;
    skos:prefLabel "Public Sector"@en .

eu-aiact:PubliclyAccessibleSpace a rdfs:Class,
        skos:Concept,
        dpv:Location ;
    dct:contributor _:person-delaram-golpayegani ;
    dct:created "2024-04-10"^^xsd:date ;
    dct:modified "2025-07-30"^^xsd:date ;
    dct:source "AIA(Art. 3(44))"@en ;
    rdfs:isDefinedBy eu-aiact: ;
    sw:term_status "modified"@en ;
    skos:broader dpv:PublicLocation ;
    skos:definition "Any publicly or privately owned physical place accessible to an undetermined number of natural persons, regardless of whether certain conditions for access may apply, and regardless of the potential capacity restrictions"@en ;
    skos:inScheme eu-aiact:misc-classes ;
    skos:prefLabel "Publicly Accessible Space"@en .

eu-aiact:PutIntoService a rdfs:Class,
        skos:Concept,
        eu-aiact:ServiceSupplyStatus ;
    dct:contributor _:person-delaram-golpayegani ;
    dct:created "2024-05-17"^^xsd:date ;
    dct:source "AIA (Art. 3(11))"@en ;
    rdfs:isDefinedBy eu-aiact: ;
    sw:term_status "accepted"@en ;
    skos:broader eu-aiact:ServiceSupplyStatus ;
    skos:definition "Status associated with the supply of an AI system for first use directly to the deployer or for own use for its intended purpose"@en ;
    skos:inScheme eu-aiact:status-classes ;
    skos:prefLabel "Put in to Service"@en .

eu-aiact:PutIntoServiceInEU a rdfs:Class,
        skos:Concept,
        eu-aiact:ServiceSupplyStatus ;
    dct:contributor _:person-delaram-golpayegani ;
    dct:created "2024-05-17"^^xsd:date ;
    dct:source "AIA (Art. 3(11))"@en ;
    rdfs:isDefinedBy eu-aiact: ;
    sw:term_status "accepted"@en ;
    skos:broader eu-aiact:PutIntoService ;
    skos:definition "Status associated with the supply of an AI system for first use directly to the deployer or for own use in the Union for its intended purpose"@en ;
    skos:inScheme eu-aiact:status-classes ;
    skos:prefLabel "Put in to Service In EU"@en .

eu-aiact:QualityManagementSystem a rdfs:Class,
        skos:Concept ;
    dct:contributor _:person-delaram-golpayegani ;
    dct:created "2026-02-09"^^xsd:date ;
    rdfs:isDefinedBy eu-aiact: ;
    rdfs:subClassOf dpv:AIGovernance,
        dpv:DataQualityManagement ;
    sw:term_status "accepted"@en ;
    skos:broader dpv:AIGovernance,
        dpv:DataQualityManagement ;
    skos:definition "A quality management system in place in relation to an AI system that ensures compliance with the AI Act"@en ;
    skos:inScheme eu-aiact:risk-classes ;
    skos:prefLabel "Quality Management System"@en .

eu-aiact:RealWorldTestSubject a rdfs:Class,
        skos:Concept ;
    dct:contributor _:person-delaram-golpayegani ;
    dct:created "2024-04-10"^^xsd:date ;
    dct:modified "2024-07-30"^^xsd:date ;
    dct:source "AIA (Art. 3(58))"@en ;
    rdfs:isDefinedBy eu-aiact: ;
    rdfs:subClassOf dpv:NaturalPerson ;
    sw:term_status "modified"@en ;
    skos:broader dpv:NaturalPerson ;
    skos:definition "A natural person who participates in testing in real world conditions"@en ;
    skos:inScheme eu-aiact:assessment-classes ;
    skos:prefLabel "Real World Test Subject"@en ;
    skos:scopeNote "Note: The term \"Real World Test Subject\" is defined as just \"Subject\" in the AI Act. We emphasise its distinction from other subjects, e.g. AI Subject, with this phrasing of the term."@en .

eu-aiact:RealWorldTestingPlan a rdfs:Class,
        skos:Concept,
        tech:Documentation ;
    dct:contributor _:person-delaram-golpayegani ;
    dct:created "2024-04-10"^^xsd:date ;
    dct:modified "2024-12-17"^^xsd:date ;
    dct:source "AIA Art.3-53"@en ;
    rdfs:isDefinedBy eu-aiact: ;
    sw:term_status "modified"@en ;
    skos:broader tech:Plan ;
    skos:definition "A document that describes the objectives, methodology, geographical, population and temporal scope, monitoring, organisation and conduct of testing in real world conditions."@en ;
    skos:inScheme eu-aiact:docs-classes ;
    skos:prefLabel "Real World Testing Plan"@en .

eu-aiact:RealtimeRemoteBiometricIdentificationSystem a rdfs:Class,
        skos:Concept,
        eu-aiact:AISystem ;
    dct:contributor _:person-delaram-golpayegani ;
    dct:created "2024-04-10"^^xsd:date ;
    dct:modified "2025-07-30"^^xsd:date ;
    dct:source "AIA(Art. 3(42))"@en ;
    rdfs:isDefinedBy eu-aiact: ;
    sw:term_status "modified"@en ;
    skos:broader eu-aiact:RemoteBiometricIdentificationSystem ;
    skos:definition "A remote biometric identification system, whereby the capturing of biometric data, the comparison and the identification all occur without a significant delay, comprising not only instant identification, but also limited short delays in order to avoid circumvention"@en ;
    skos:inScheme eu-aiact:system-classes ;
    skos:prefLabel "Real-time Remote Biometric Identification System"@en ;
    skos:related pd:Biometric .

eu-aiact:ReasonablyForeseeableMisuse a rdfs:Class,
        skos:Concept,
        dpv:RiskConcept ;
    dct:contributor _:person-arthit-suriyawongkul,
        _:person-delaram-golpayegani,
        _:person-georg-p-krog,
        _:person-harshvardhan-j-pandit ;
    dct:created "2024-04-10"^^xsd:date ;
    dct:modified "2025-06-19"^^xsd:date ;
    dct:source "AIA (Art. 3(13))"@en ;
    rdfs:isDefinedBy eu-aiact: ;
    sw:term_status "modified"@en ;
    skos:broader risk:Misuse ;
    skos:definition "The use of an AI system in a way that is not in accordance with its intended purpose, but which may result from reasonably foreseeable human behaviour or interaction with other systems, including other AI systems"@en ;
    skos:inScheme eu-aiact:risk-classes ;
    skos:prefLabel "Reasonably Foreseeable Misuse"@en ;
    skos:scopeNote "Misuse should be provided through the Risk extension, along with taxonomy e.g. Misuse -> Foreseeable -> Reasonably and NonReasonably Foreseeable; and Misuse -> Unforeseeable Misuse."@en .

eu-aiact:RecalledFromService a rdfs:Class,
        skos:Concept,
        eu-aiact:ServiceSupplyStatus ;
    dct:contributor _:person-delaram-golpayegani ;
    dct:created "2024-05-17"^^xsd:date ;
    rdfs:isDefinedBy eu-aiact: ;
    sw:term_status "accepted"@en ;
    skos:broader eu-aiact:ServiceSupplyStatus ;
    skos:definition "An AI system that is returned to the provider or taken out of service or use"@en ;
    skos:inScheme eu-aiact:status-classes ;
    skos:prefLabel "Recalled from Service"@en .

eu-aiact:RemoteBiometricIdentificationSystem a rdfs:Class,
        skos:Concept,
        eu-aiact:AISystem ;
    dct:contributor _:person-delaram-golpayegani ;
    dct:created "2024-04-10"^^xsd:date ;
    dct:modified "2025-07-30"^^xsd:date ;
    dct:source "AIA(Art. 3(41))"@en ;
    rdfs:isDefinedBy eu-aiact: ;
    sw:term_status "modified"@en ;
    skos:broader eu-aiact:AISystem ;
    skos:definition "An AI system for the purpose of identifying natural persons, without their active involvement, typically at a distance through the comparison of a person’s biometric data with the biometric data contained in a reference database."@en ;
    skos:inScheme eu-aiact:system-classes ;
    skos:prefLabel "Remote Biometric Identification System"@en ;
    skos:related pd:Biometric .

eu-aiact:Risk a rdfs:Class,
        skos:Concept ;
    dct:contributor _:person-delaram-golpayegani ;
    dct:created "2024-04-10"^^xsd:date ;
    dct:modified "2025-07-30"^^xsd:date ;
    dct:source "AIA (Art. 3(2))"@en ;
    rdfs:isDefinedBy eu-aiact: ;
    rdfs:subClassOf dpv:Risk ;
    sw:term_status "modified"@en ;
    skos:broader dpv:Risk ;
    skos:definition "The combination of the probability of an occurrence of harm and the severity of that harm"@en ;
    skos:inScheme eu-aiact:risk-classes ;
    skos:prefLabel "Risk"@en .

eu-aiact:RiskLevel a rdfs:Class,
        skos:Concept ;
    dct:contributor _:person-arthit-suriyawongkul,
        _:person-delaram-golpayegani,
        _:person-georg-p-krog,
        _:person-harshvardhan-j-pandit ;
    dct:created "2025-04-03"^^xsd:date ;
    dct:source "AI Act"@en ;
    rdfs:isDefinedBy eu-aiact: ;
    rdfs:subClassOf dpv:RiskLevel ;
    sw:term_status "accepted"@en ;
    skos:broader dpv:RiskLevel ;
    skos:definition "Enumeration of AI Act's risk-based categorisation which determines the prohibitions and obligations for AI systems"@en ;
    skos:inScheme eu-aiact:risk-levels-classes ;
    skos:prefLabel "Risk Level"@en .

eu-aiact:RiskLevelHigh a rdfs:Class,
        skos:Concept,
        eu-aiact:RiskLevel ;
    dct:contributor _:person-arthit-suriyawongkul,
        _:person-delaram-golpayegani,
        _:person-georg-p-krog,
        _:person-harshvardhan-j-pandit ;
    dct:created "2025-04-03"^^xsd:date ;
    dct:source "AIA(Art.6)"@en ;
    rdfs:isDefinedBy eu-aiact: ;
    sw:term_status "accepted"@en ;
    skos:broader eu-aiact:RiskLevelPermitted ;
    skos:definition "Risk Level categorising an AI system as \"high-risk\" as defined in the AI Act Article 6"@en ;
    skos:inScheme eu-aiact:risk-levels-classes ;
    skos:prefLabel "Risk Level - High"@en .

eu-aiact:RiskLevelHigh-A6-1 a rdfs:Class,
        skos:Concept,
        eu-aiact:RiskLevel ;
    dct:contributor _:person-delaram-golpayegani,
        _:person-harshvardhan-j-pandit ;
    dct:created "2026-02-09"^^xsd:date ;
    dct:source "AIA(Art.6(1))"@en ;
    rdfs:isDefinedBy eu-aiact: ;
    sw:term_status "accepted"@en ;
    skos:broader eu-aiact:RiskLevelHigh ;
    skos:definition "Risk Level categorising an AI system as \"high-risk\" as defined in the AI Act Article 6(1), which specifies the sectorial laws mentiond in Annex I"@en ;
    skos:inScheme eu-aiact:risk-levels-classes ;
    skos:prefLabel "Risk Level - High per Article 6(1)"@en .

eu-aiact:RiskLevelHigh-A6-2 a rdfs:Class,
        skos:Concept,
        eu-aiact:RiskLevel ;
    dct:contributor _:person-delaram-golpayegani,
        _:person-harshvardhan-j-pandit ;
    dct:created "2026-02-09"^^xsd:date ;
    dct:source "AIA(Art.6(2))"@en ;
    rdfs:isDefinedBy eu-aiact: ;
    sw:term_status "accepted"@en ;
    skos:broader eu-aiact:RiskLevelHigh ;
    skos:definition "Risk Level categorising an AI system as \"high-risk\" as defined in the AI Act Article 6(1), which specifies applications of AI in Annex III"@en ;
    skos:inScheme eu-aiact:risk-levels-classes ;
    skos:prefLabel "Risk Level - High per Article 6(2)"@en .

eu-aiact:RiskLevelMinimal a rdfs:Class,
        skos:Concept,
        eu-aiact:RiskLevel ;
    dct:contributor _:person-arthit-suriyawongkul,
        _:person-delaram-golpayegani,
        _:person-georg-p-krog,
        _:person-harshvardhan-j-pandit ;
    dct:created "2025-04-03"^^xsd:date ;
    rdfs:isDefinedBy eu-aiact: ;
    sw:term_status "accepted"@en ;
    skos:broader eu-aiact:RiskLevelNotHigh ;
    skos:definition "Risk Level categorising an AI system as not being prohibited or high-risk or transparency required as defined in the AI Act"@en ;
    skos:inScheme eu-aiact:risk-levels-classes ;
    skos:prefLabel "Risk Level - Minimal"@en ;
    skos:scopeNote "The minimal risk level does not indicate there is no risk, but instead indicates that it is not sufficient to be regulated under the categorisations of the AI Act"@en .

eu-aiact:RiskLevelNotHigh a rdfs:Class,
        skos:Concept,
        eu-aiact:RiskLevel ;
    dct:contributor _:person-arthit-suriyawongkul,
        _:person-delaram-golpayegani,
        _:person-georg-p-krog,
        _:person-harshvardhan-j-pandit ;
    dct:created "2025-04-03"^^xsd:date ;
    rdfs:isDefinedBy eu-aiact: ;
    sw:term_status "accepted"@en ;
    skos:broader eu-aiact:RiskLevelPermitted ;
    skos:definition "Risk Level categorising an AI system as not being \"high-risk\" as defined in the AI Act"@en ;
    skos:inScheme eu-aiact:risk-levels-classes ;
    skos:prefLabel "Risk Level - Not High"@en ;
    skos:scopeNote "The \"not high\" risk level is useful for indicating the outcomes of assessments determining whether something is high-risk"@en .

eu-aiact:RiskLevelPermitted a rdfs:Class,
        skos:Concept,
        eu-aiact:RiskLevel ;
    dct:contributor _:person-arthit-suriyawongkul,
        _:person-delaram-golpayegani,
        _:person-georg-p-krog,
        _:person-harshvardhan-j-pandit ;
    dct:created "2025-04-03"^^xsd:date ;
    rdfs:isDefinedBy eu-aiact: ;
    sw:term_status "accepted"@en ;
    skos:broader eu-aiact:RiskLevel ;
    skos:definition "Risk Level representing \"AI practices\" are permitted i.e. not prohibited under the AI Act"@en ;
    skos:inScheme eu-aiact:risk-levels-classes ;
    skos:prefLabel "Risk Level - Permitted"@en ;
    skos:scopeNote "The permitted risk level is useful for representing outcomes of assessments determining whether something is prohibited"@en .

eu-aiact:RiskLevelProhibited a rdfs:Class,
        skos:Concept,
        eu-aiact:RiskLevel ;
    dct:contributor _:person-arthit-suriyawongkul,
        _:person-delaram-golpayegani,
        _:person-georg-p-krog,
        _:person-harshvardhan-j-pandit ;
    dct:created "2025-04-03"^^xsd:date ;
    dct:source "AIA(Art.5)"@en ;
    rdfs:isDefinedBy eu-aiact: ;
    sw:term_status "accepted"@en ;
    skos:broader eu-aiact:RiskLevel ;
    skos:definition "Risk Level prohibiting \"AI practices\" as defined in the AI Act Article 5"@en ;
    skos:inScheme eu-aiact:risk-levels-classes ;
    skos:prefLabel "Risk Level - Prohibited"@en .

eu-aiact:RiskLevelTransparencyRequired a rdfs:Class,
        skos:Concept,
        eu-aiact:RiskLevel ;
    dct:contributor _:person-arthit-suriyawongkul,
        _:person-delaram-golpayegani,
        _:person-georg-p-krog,
        _:person-harshvardhan-j-pandit ;
    dct:created "2025-04-03"^^xsd:date ;
    dct:source "AIA(Art.50)"@en ;
    rdfs:isDefinedBy eu-aiact: ;
    sw:term_status "accepted"@en ;
    skos:broader eu-aiact:RiskLevelNotHigh ;
    skos:definition "Risk Level categorising an AI system as not high-risk but where transparency is require as defined in the AI Act"@en ;
    skos:inScheme eu-aiact:risk-levels-classes ;
    skos:prefLabel "Risk Level - Transparency Required"@en .

eu-aiact:RiskManagementSystem a rdfs:Class,
        skos:Concept ;
    dct:contributor _:person-delaram-golpayegani ;
    dct:created "2024-06-12"^^xsd:date ;
    dct:source "AI Act"@en ;
    rdfs:isDefinedBy eu-aiact: ;
    rdfs:subClassOf risk:RiskManagement ;
    sw:term_status "accepted"@en ;
    skos:broader risk:RiskManagement ;
    skos:definition "A risk management system is a continuous iterative process planned and run throughout the entire lifecycle of a high-risk AI system, requiring regular systematic review and updating"@en ;
    skos:inScheme eu-aiact:risk-classes ;
    skos:prefLabel "Risk Management System"@en .

eu-aiact:SafetyComponent a rdfs:Class,
        skos:Concept ;
    dct:contributor _:person-delaram-golpayegani ;
    dct:created "2024-04-10"^^xsd:date ;
    dct:modified "2025-07-30"^^xsd:date ;
    dct:source "AIA (Art. 3(14))"@en ;
    rdfs:isDefinedBy eu-aiact: ;
    rdfs:subClassOf tech:Component ;
    sw:term_status "modified"@en ;
    skos:broader tech:Component ;
    skos:definition "A component of a product or of an AI system which fulfils a safety function for that product or AI system, or the failure or malfunctioning of which endangers the health and safety of persons or property"@en ;
    skos:inScheme eu-aiact:system-classes ;
    skos:prefLabel "Safety Component"@en .

eu-aiact:SandboxPlan a rdfs:Class,
        skos:Concept,
        tech:Documentation ;
    dct:contributor _:person-delaram-golpayegani ;
    dct:created "2024-04-10"^^xsd:date ;
    dct:modified "2025-07-31"^^xsd:date ;
    dct:source "AIA (Art.3(54))"@en ;
    rdfs:isDefinedBy eu-aiact: ;
    sw:term_status "modified"@en ;
    skos:broader tech:Plan ;
    skos:definition "A document agreed between the participating provider and the competent authority describing the objectives, conditions, timeframe, methodology and requirements for the activities carried out within the sandbox"@en ;
    skos:inScheme eu-aiact:docs-classes ;
    skos:prefLabel "Sandbox Plan"@en .

eu-aiact:SeriousIncident a rdfs:Class,
        skos:Concept ;
    dct:contributor _:person-delaram-golpayegani ;
    dct:created "2024-04-10"^^xsd:date ;
    dct:modified "2025-07-30"^^xsd:date ;
    dct:source "AIA (Art. 3(49))"@en ;
    rdfs:isDefinedBy eu-aiact: ;
    rdfs:subClassOf risk:Incident ;
    sw:term_status "modified"@en ;
    skos:broader risk:Incident ;
    skos:definition """an incident or malfunctioning of an AI system that directly or indirectly leads to any of the following:
(a) the death of a person, or serious harm to a person’s health;
(b) a serious and irreversible disruption of the management or operation of critical infrastructure;
(c) the infringement of obligations under Union law intended to protect fundamental rights;
(d) serious harm to property or the environment;"""@en ;
    skos:inScheme eu-aiact:risk-classes ;
    skos:prefLabel "Serious Incident"@en .

eu-aiact:ServiceSupplyStatus a rdfs:Class,
        skos:Concept ;
    dct:contributor _:person-delaram-golpayegani ;
    dct:created "2024-05-17"^^xsd:date ;
    rdfs:isDefinedBy eu-aiact: ;
    rdfs:subClassOf tech:ProvisionStatus ;
    sw:term_status "accepted"@en ;
    skos:broader tech:ProvisionStatus ;
    skos:definition "Status associated with whether the AI system has been supplied for use or put in to service or been recalled or withdrawn"@en ;
    skos:inScheme eu-aiact:status-classes ;
    skos:prefLabel "Service Supply Status"@en .

eu-aiact:SubliminalCapability a rdfs:Class,
        skos:Concept,
        tech:Capability ;
    dct:contributor _:person-delaram-golpayegani ;
    dct:created "2026-02-09"^^xsd:date ;
    dct:source " Commission guidelines on prohibited AI practices established by AI Act"@en,
        "AIA Art.5(1)"@en ;
    rdfs:isDefinedBy eu-aiact: ;
    sw:term_status "accepted"@en ;
    skos:broader ai:HumanOrientedCapability ;
    skos:definition "Capability that operates beyond (below or above) the threshold of conscious awareness"@en ;
    skos:inScheme eu-aiact:capability-classes ;
    skos:prefLabel "Subliminal Capability"@en .

eu-aiact:SubstantialModification a rdfs:Class,
        skos:Concept ;
    dct:contributor _:person-delaram-golpayegani ;
    dct:created "2024-04-10"^^xsd:date ;
    dct:modified "2025-07-30"^^xsd:date ;
    dct:source "AIA(Art. 3(23))"@en ;
    rdfs:isDefinedBy eu-aiact: ;
    sw:term_status "modified"@en ;
    skos:definition "A change to an AI system after its placing on the market or putting into service which is not foreseen or planned in the initial conformity assessment carried out by the provider and as a result of which the compliance of the AI system with the requirements set out in Chapter III, Section 2 is affected or results in a modification to the intended purpose for which the AI system has been assessed"@en ;
    skos:inScheme eu-aiact:misc-classes ;
    skos:prefLabel "Substantial Modification"@en .

eu-aiact:SystemArchitectureDescription a rdfs:Class,
        skos:Concept,
        tech:Documentation ;
    dct:contributor _:person-delaram-golpayegani ;
    dct:created "2024-12-01"^^xsd:date ;
    dct:source "AI Act Annex.IV"@en ;
    rdfs:isDefinedBy eu-aiact: ;
    sw:term_status "accepted"@en ;
    skos:broader tech:Documentation ;
    skos:definition "Documentation specifying the software architecture"@en ;
    skos:inScheme eu-aiact:docs-classes ;
    skos:prefLabel "System Architecture Description"@en .

eu-aiact:SystemicRisk a rdfs:Class,
        skos:Concept ;
    dct:contributor _:person-delaram-golpayegani ;
    dct:created "2024-04-10"^^xsd:date ;
    dct:modified "2025-07-30"^^xsd:date ;
    dct:source "AIA(Art.3 (65))"@en ;
    rdfs:isDefinedBy eu-aiact: ;
    rdfs:subClassOf eu-aiact:Risk ;
    sw:term_status "modified"@en ;
    skos:broader eu-aiact:Risk ;
    skos:definition "Q risk that is specific to the high-impact capabilities of general-purpose AI models, having a significant impact on the Union market due to their reach, or due to actual or reasonably foreseeable negative effects on public health, safety, public security, fundamental rights, or the society as a whole, that can be propagated at scale across the value chain"@en ;
    skos:inScheme eu-aiact:risk-classes ;
    skos:prefLabel "Systemic Risk"@en .

eu-aiact:TechnicalDocumentation a rdfs:Class,
        skos:Concept,
        tech:Documentation ;
    dct:contributor _:person-delaram-golpayegani ;
    dct:created "2024-04-10"^^xsd:date ;
    dct:modified "2024-12-17"^^xsd:date ;
    dct:source " AIA Annex.IV"@en,
        "AIA Art.11"@en ;
    rdfs:isDefinedBy eu-aiact: ;
    sw:term_status "modified"@en ;
    skos:broader tech:Documentation ;
    skos:definition "Annex IV technical documentation"@en ;
    skos:inScheme eu-aiact:docs-classes ;
    skos:prefLabel "Technical Documentation"@en .

eu-aiact:TestLog a rdfs:Class,
        skos:Concept,
        tech:Documentation ;
    dct:contributor _:person-delaram-golpayegani ;
    dct:created "2024-12-01"^^xsd:date ;
    dct:source "AI Act Annex.IV"@en ;
    rdfs:isDefinedBy eu-aiact: ;
    sw:term_status "accepted"@en ;
    skos:broader tech:Documentation ;
    skos:definition "Log of the tests performed"@en ;
    skos:inScheme eu-aiact:docs-classes ;
    skos:prefLabel "Test Log"@en .

eu-aiact:TestReport a rdfs:Class,
        skos:Concept,
        tech:Documentation ;
    dct:contributor _:person-delaram-golpayegani ;
    dct:created "2024-12-01"^^xsd:date ;
    dct:source "AI Act Annex.IV"@en ;
    rdfs:isDefinedBy eu-aiact: ;
    sw:term_status "accepted"@en ;
    skos:broader tech:Documentation ;
    skos:definition "A document that includes a summary of test activities and their results"@en ;
    skos:inScheme eu-aiact:docs-classes ;
    skos:prefLabel "Test Report"@en .

eu-aiact:TestingData a rdfs:Class,
        skos:Concept ;
    dct:contributor _:person-delaram-golpayegani ;
    dct:created "2024-04-10"^^xsd:date ;
    dct:modified "2025-07-30"^^xsd:date ;
    dct:source "AIA (Art. 3(32))"@en ;
    rdfs:isDefinedBy eu-aiact: ;
    rdfs:subClassOf ai:TestingData ;
    sw:term_status "modified"@en ;
    skos:broader ai:TestingData ;
    skos:definition "Data used for providing an independent evaluation of the AI system in order to confirm the expected performance of that system before its placing on the market or putting into service"@en ;
    skos:inScheme eu-aiact:data-classes ;
    skos:prefLabel "Testing Data"@en .

eu-aiact:TestingRealWorldConditions a rdfs:Class,
        skos:Concept,
        dpv:OrganisationalMeasure ;
    dct:contributor _:person-delaram-golpayegani ;
    dct:created "2024-04-10"^^xsd:date ;
    dct:modified "2024-07-30"^^xsd:date ;
    dct:source "AIA (Art. 3(57))"@en ;
    rdfs:isDefinedBy eu-aiact: ;
    sw:term_status "modified"@en ;
    skos:broader dpv:OrganisationalMeasure ;
    skos:definition "The temporary testing of an AI system for its intended purpose in real-world conditions outside a laboratory or otherwise simulated environment, with a view to gathering reliable and robust data and to assessing and verifying the conformity of the AI system with the requirements of the AI Act and it does not qualify as placing the AI system on the market or putting it into service within the meaning of the AI Act, provided that all the conditions laid down in Article 57 or 60 are fulfilled"@en ;
    skos:inScheme eu-aiact:assessment-classes ;
    skos:prefLabel "Testing In Real World Conditions"@en .

eu-aiact:TrainingData a rdfs:Class,
        skos:Concept ;
    dct:contributor _:person-delaram-golpayegani ;
    dct:created "2024-04-10"^^xsd:date ;
    dct:modified "2024-12-01"^^xsd:date ;
    dct:source "AIA(Art. 3(29))"@en ;
    rdfs:isDefinedBy eu-aiact: ;
    rdfs:subClassOf ai:TrainingData ;
    sw:term_status "modified"@en ;
    skos:broader ai:TrainingData ;
    skos:definition "Data used for training an AI system through fitting its learnable parameters"@en ;
    skos:inScheme eu-aiact:data-classes ;
    skos:prefLabel "Training Data"@en .

eu-aiact:ValidationData a rdfs:Class,
        skos:Concept ;
    dct:contributor _:person-delaram-golpayegani ;
    dct:created "2024-04-10"^^xsd:date ;
    dct:modified "2025-07-30"^^xsd:date ;
    dct:source "AIA (Art. 3(30))"@en ;
    rdfs:isDefinedBy eu-aiact: ;
    rdfs:subClassOf ai:ValidationData ;
    sw:term_status "modified"@en ;
    skos:broader ai:ValidationData ;
    skos:definition "Data used for providing an evaluation of the trained AI system and for tuning its non-learnable parameters and its learning process in order, inter alia, to prevent underfitting or overfitting"@en ;
    skos:inScheme eu-aiact:data-classes ;
    skos:prefLabel "Validation Data"@en .

eu-aiact:WithdrawnFromService a rdfs:Class,
        skos:Concept,
        eu-aiact:ServiceSupplyStatus ;
    dct:contributor _:person-delaram-golpayegani ;
    dct:created "2024-05-17"^^xsd:date ;
    rdfs:isDefinedBy eu-aiact: ;
    sw:term_status "accepted"@en ;
    skos:broader eu-aiact:ServiceSupplyStatus ;
    skos:definition "An AI system that is prevented to be made available in the supply chain"@en ;
    skos:inScheme eu-aiact:status-classes ;
    skos:prefLabel "Withdrawn from Service"@en .

<https://w3id.org/dpv/legal/eu/aiact> a owl:Ontology,
        profile:Profile ;
    dct:bibliographicCitation "Harshvardhan J. Pandit, Beatriz Esteves, Georg P. Krog, Paul Ryan, Delaram Golpayegani, Julian Flake (2025) Data Privacy Vocabulary (DPV) – Version 2.0. In: Demartini, G., et al. The Semantic Web – ISWC 2024. ISWC 2024. Lecture Notes in Computer Science, vol 15233. Springer, Cham. https://doi.org/10.1007/978-3-031-77847-6_10" ;
    dct:conformsTo "http://www.w3.org/2000/01/rdf-schema",
        "http://www.w3.org/2004/02/skos/core" ;
    dct:contributor _:person-arthit-suriyawongkul,
        _:person-beatriz-esteves,
        _:person-delaram-golpayegani,
        _:person-georg-p-krog,
        _:person-harshvardhan-j-pandit ;
    dct:created "2024-04-10"@en ;
    dct:creator _:person-delaram-golpayegani ;
    dct:description "Extension to the Data Privacy Vocabulary (DPV) providing concepts for representing information associated with EU AI Act"@en ;
    dct:identifier "https://w3id.org/dpv/legal/eu/aiact" ;
    dct:issued "2024-04-10"@en ;
    dct:license <https://www.w3.org/copyright/document-license-2023/> ;
    dct:modified "2026-02-25"@en ;
    dct:publisher <https://www.w3.org/> ;
    dct:source <https://www.w3.org/groups/cg/dpvcg/> ;
    dct:title "EU Artificial Intelligence Act (AI Act)"@en ;
    bibo:doi "10.5281/zenodo.12505841" ;
    bibo:status "http://purl.org/ontology/bibo/status/published" ;
    vann:preferredNamespacePrefix "eu-aiact" ;
    vann:preferredNamespaceUri "https://w3id.org/dpv/legal/eu/aiact#" ;
    rdfs:Label "EU-AIACT"@en ;
    owl:versionIRI <https://w3id.org/dpv/2.3/legal/eu/aiact> ;
    owl:versionInfo "2.3" ;
    profile:hasResource <https://w3id.org/dpv/examples>,
        <https://w3id.org/dpv/guides>,
        eu-aiact:serialisation-html,
        eu-aiact:serialisation-ttl,
        <https://w3id.org/dpv/primer> ;
    profile:isProfileOf rdfs:,
        skos:,
        <https://w3id.org/dpv> ;
    foaf:logo <https://w3id.org/dpv/media/logo.png> ;
    schema:version "2.3" .

eu-aiact:hasChangeCategory a rdf:Property,
        skos:Concept ;
    dcam:domainIncludes tech:AI ;
    dcam:rangeIncludes eu-aiact:ChangeCategory ;
    dct:contributor _:person-delaram-golpayegani ;
    dct:created "2024-12-01"^^xsd:date ;
    rdfs:isDefinedBy eu-aiact: ;
    rdfs:subPropertyOf dpv:hasContext ;
    sw:term_status "accepted"@en ;
    skos:broader dpv:hasContext ;
    skos:definition "Associates the category of change to the AI"@en ;
    skos:inScheme eu-aiact:status-properties ;
    skos:prefLabel "has change category"@en ;
    schema:domainIncludes tech:AI ;
    schema:rangeIncludes eu-aiact:ChangeCategory .

eu-aiact:hasChangeDescription a rdf:Property,
        skos:Concept ;
    dcam:domainIncludes tech:AI ;
    dcam:rangeIncludes eu-aiact:ChangeDescription ;
    dct:contributor _:person-delaram-golpayegani ;
    dct:created "2024-12-01"^^xsd:date ;
    rdfs:isDefinedBy eu-aiact: ;
    rdfs:subPropertyOf dpv:hasContext ;
    sw:term_status "accepted"@en ;
    skos:broader dpv:hasContext ;
    skos:definition "Associates the change description to AI"@en ;
    skos:inScheme eu-aiact:status-properties ;
    skos:prefLabel "has change description"@en ;
    schema:domainIncludes tech:AI ;
    schema:rangeIncludes eu-aiact:ChangeDescription .

eu-aiact:hasRiskLevel a rdf:Property,
        skos:Concept ;
    dcam:domainIncludes eu-aiact:AISystem ;
    dcam:rangeIncludes eu-aiact:RiskLevel ;
    dct:contributor _:person-harshvardhan-j-pandit ;
    dct:created "2026-02-09"^^xsd:date ;
    rdfs:isDefinedBy eu-aiact: ;
    rdfs:subPropertyOf dpv:hasRiskLevel ;
    sw:term_status "accepted"@en ;
    skos:broader dpv:hasRiskLevel ;
    skos:definition "Indicates the risk level of the AI system under the AI Act"@en ;
    skos:inScheme eu-aiact:risk-levels-properties ;
    skos:prefLabel "has risk level"@en ;
    schema:domainIncludes eu-aiact:AISystem ;
    schema:rangeIncludes eu-aiact:RiskLevel .

eu-aiact:risk-levels-properties a skos:ConceptScheme .

eu-aiact:serialisation-html a profile:ResourceDescriptor ;
    dct:conformsTo <https://www.w3.org/TR/html/> ;
    dct:format <https://www.iana.org/assignments/media-types/text/html> ;
    dct:title "EU Artificial Intelligence Act (AI Act) - HTML serialisation" ;
    profile:hasArtifact <https://w3id.org/dpv/legal/eu/aiact/eu-aiact.html> ;
    profile:hasRole role:specification .

eu-aiact:serialisation-ttl a profile:ResourceDescriptor ;
    dct:conformsTo <https://www.w3.org/TR/turtle/> ;
    dct:format <https://www.iana.org/assignments/media-types/text/turtle> ;
    dct:title "EU Artificial Intelligence Act (AI Act) - Turtle serialisation" ;
    profile:hasArtifact <https://w3id.org/dpv/legal/eu/aiact/eu-aiact.ttl> ;
    profile:hasRole role:vocabulary .

<https://w3id.org/dpv/examples> a profile:ResourceDescriptor ;
    dct:conformsTo <https://www.w3.org/TR/html/> ;
    dct:format <https://www.iana.org/assignments/media-types/text/html> ;
    dct:title "Examples" ;
    profile:hasArtifact <https://w3id.org/dpv/examples> ;
    profile:hasRole role:guidance .

<https://w3id.org/dpv/guides> a profile:ResourceDescriptor ;
    dct:conformsTo <https://www.w3.org/TR/html/> ;
    dct:format <https://www.iana.org/assignments/media-types/text/html> ;
    dct:title "Guides for Data Privacy Vocabulary" ;
    profile:hasArtifact <https://w3id.org/dpv/guides> ;
    profile:hasRole role:guidance .

eu-aiact:status-properties a skos:ConceptScheme .

<https://w3id.org/dpv/primer> a profile:ResourceDescriptor ;
    dct:conformsTo <https://www.w3.org/TR/html/> ;
    dct:format <https://www.iana.org/assignments/media-types/text/html> ;
    dct:title "Primer for Data Privacy Vocabulary" ;
    profile:hasArtifact <https://w3id.org/dpv/primer> ;
    profile:hasRole role:guidance .

eu-aiact:compliance-classes a skos:ConceptScheme .

eu-aiact:data-classes a skos:ConceptScheme .

eu-aiact:misc-classes a skos:ConceptScheme .

eu-aiact:capability-classes a skos:ConceptScheme .

eu-aiact:prohibited-systems-classes a skos:ConceptScheme .

eu-aiact:risk-classes a skos:ConceptScheme .

eu-aiact:risk-levels-classes a skos:ConceptScheme .

eu-aiact:assessment-classes a skos:ConceptScheme .

eu-aiact:docs-classes a skos:ConceptScheme .

eu-aiact:sector-classes a skos:ConceptScheme .

eu-aiact:system-classes a skos:ConceptScheme .

eu-aiact:roles-classes a skos:ConceptScheme .

eu-aiact:status-classes a skos:ConceptScheme .

eu-aiact:highrisk-systems-classes a skos:ConceptScheme .

_:org-ai-accountability-lab-aial-trinity-college-dublin a foaf:Organization ;
    foaf:name "AI Accountability Lab (AIAL), Trinity College Dublin" .

_:org-idlab-imec-ghent-university a foaf:Organization ;
    foaf:name "IDLab, IMEC, Ghent University" .

_:org-signatu-as a foaf:Organization ;
    foaf:name "Signatu AS" .

_:org-adapt-centre-trinity-college-dublin a foaf:Organization ;
    foaf:name "ADAPT Centre, Trinity College Dublin" .

_:person-beatriz-esteves a dct:Agent,
        foaf:Person ;
    scoro:hasORCID "0000-0003-0259-7560" ;
    org:memberOf _:org-idlab-imec-ghent-university ;
    foaf:homepage "https://w3id.org/people/besteves" ;
    foaf:name "Beatriz Esteves" .

_:person-arthit-suriyawongkul a dct:Agent,
        foaf:Person ;
    scoro:hasORCID "0000-0002-9698-1899" ;
    org:memberOf _:org-adapt-centre-trinity-college-dublin ;
    foaf:name "Arthit Suriyawongkul" .

_:person-georg-p-krog a dct:Agent,
        foaf:Person ;
    org:memberOf _:org-signatu-as ;
    foaf:homepage "https://www.linkedin.com/in/georg-philip-krog-a2a278104/" ;
    foaf:name "Georg P. Krog" .

_:person-harshvardhan-j-pandit a dct:Agent,
        foaf:Person ;
    scoro:hasORCID "0000-0002-5068-3714" ;
    org:memberOf _:org-ai-accountability-lab-aial-trinity-college-dublin ;
    foaf:homepage "https://harshp.com/" ;
    foaf:name "Harshvardhan J. Pandit" .

_:person-delaram-golpayegani a dct:Agent,
        foaf:Person ;
    scoro:hasORCID "0000-0002-1208-186X" ;
    org:memberOf _:org-adapt-centre-trinity-college-dublin ;
    foaf:name "Delaram Golpayegani" .

