@prefix bibo: <http://purl.org/ontology/bibo/> .
@prefix dct: <http://purl.org/dc/terms/> .
@prefix dpv: <https://w3id.org/dpv#> .
@prefix foaf: <http://xmlns.com/foaf/0.1/> .
@prefix org: <http://www.w3.org/ns/org#> .
@prefix owl: <http://www.w3.org/2002/07/owl#> .
@prefix profile: <http://www.w3.org/ns/dx/prof/> .
@prefix rdf: <http://www.w3.org/1999/02/22-rdf-syntax-ns#> .
@prefix rdfs: <http://www.w3.org/2000/01/rdf-schema#> .
@prefix role: <http://www.w3.org/ns/dx/prof/role/> .
@prefix schema: <https://schema.org/> .
@prefix scoro: <http://purl.org/spar/scoro/> .
@prefix sector-infra: <https://w3id.org/dpv/sector/infra#> .
@prefix sector-law: <https://w3id.org/dpv/sector/law#> .
@prefix skos: <http://www.w3.org/2004/02/skos/core#> .
@prefix sw: <http://www.w3.org/2003/06/sw-vocab-status/ns#> .
@prefix vann: <http://purl.org/vocab/vann/> .
@prefix xsd: <http://www.w3.org/2001/XMLSchema#> .

sector-law:CrimeArrestDetention a rdfs:Class,
        skos:Concept,
        dpv:Purpose ;
    dct:created "2024-12-01"^^xsd:date ;
    rdfs:isDefinedBy sector-law: ;
    sw:term_status "accepted"@en ;
    skos:broader sector-law:CriminalLawEnforcement ;
    skos:definition "Purposes associated with arresting and detention of individuals in relation to criminal activities within the legal system"@en ;
    skos:inScheme sector-law:purposes-classes ;
    skos:prefLabel "Crime Arrest Detention"@en .

sector-law:CrimeDetection a rdfs:Class,
        skos:Concept,
        dpv:Purpose ;
    dct:created "2024-12-01"^^xsd:date ;
    rdfs:isDefinedBy sector-law: ;
    sw:term_status "accepted"@en ;
    skos:broader sector-law:CriminalLawEnforcement,
        sector-law:LegalOffenceDetection ;
    skos:definition "Purposes associated with detection of crimes within the legal system"@en ;
    skos:inScheme sector-law:purposes-classes ;
    skos:prefLabel "Crime Detection"@en .

sector-law:CrimeInvestigation a rdfs:Class,
        skos:Concept,
        dpv:Purpose ;
    dct:created "2024-12-01"^^xsd:date ;
    rdfs:isDefinedBy sector-law: ;
    sw:term_status "accepted"@en ;
    skos:broader sector-law:CriminalLawEnforcement,
        sector-law:LegalInvestigation ;
    skos:definition "Purposes associated with investigation of crimes within the legal system"@en ;
    skos:inScheme sector-law:purposes-classes ;
    skos:prefLabel "Crime Investigation"@en .

sector-law:CrimeProsecution a rdfs:Class,
        skos:Concept,
        dpv:Purpose ;
    dct:created "2024-12-01"^^xsd:date ;
    rdfs:isDefinedBy sector-law: ;
    sw:term_status "accepted"@en ;
    skos:broader sector-law:CriminalLawEnforcement,
        sector-law:LegalOffenceProsecution ;
    skos:definition "Purposes associated with prosecution of criminal activities within the legal system"@en ;
    skos:inScheme sector-law:purposes-classes ;
    skos:prefLabel "Crime Prosecution"@en .

sector-law:CrimeSurveillance a rdfs:Class,
        skos:Concept,
        dpv:Purpose ;
    dct:created "2024-12-01"^^xsd:date ;
    rdfs:isDefinedBy sector-law: ;
    sw:term_status "accepted"@en ;
    skos:broader sector-law:CriminalLawEnforcement,
        sector-law:LegalOffenceSurveillance ;
    skos:definition "Purposes associated with monitoring or observing to detect or deter potential or ongoing criminal activities within the legal system"@en ;
    skos:inScheme sector-law:purposes-classes ;
    skos:prefLabel "Crime Surveillance"@en .

sector-law:CrimeVictimCounsellingManagement a rdfs:Class,
        skos:Concept,
        dpv:Purpose ;
    dct:created "2024-12-01"^^xsd:date ;
    rdfs:isDefinedBy sector-law: ;
    sw:term_status "accepted"@en ;
    skos:broader sector-law:CrimeVictimSafetyManagement ;
    skos:definition "Purposes associated with management of counselling for victims of criminal activities within the legal system"@en ;
    skos:inScheme sector-law:purposes-classes ;
    skos:prefLabel "Crime Victim Counselling Management"@en .

sector-law:CrimeVictimPrediction a rdfs:Class,
        skos:Concept,
        dpv:Purpose ;
    dct:created "2024-12-01"^^xsd:date ;
    rdfs:isDefinedBy sector-law: ;
    sw:term_status "accepted"@en ;
    skos:broader sector-law:CrimeVictimSafetyManagement ;
    skos:definition "Purposes associated with predicting safety concerns or threats for victims of criminal activities within the legal system"@en ;
    skos:inScheme sector-law:purposes-classes ;
    skos:prefLabel "Crime Victim Prediction"@en .

sector-law:CrimeVictimRestitutionSupport a rdfs:Class,
        skos:Concept,
        dpv:Purpose ;
    dct:created "2024-12-01"^^xsd:date ;
    rdfs:isDefinedBy sector-law: ;
    sw:term_status "accepted"@en ;
    skos:broader sector-law:CrimeVictimSafetyManagement ;
    skos:definition "Purposes associated with supporting victims of criminal activities through restitution or providing restoration or compensation of goods and services within the legal system"@en ;
    skos:inScheme sector-law:purposes-classes ;
    skos:prefLabel "Crime Victim Restitution Support"@en .

sector-law:CrimeVictimSafetyAssessment a rdfs:Class,
        skos:Concept,
        dpv:Purpose ;
    dct:created "2024-12-01"^^xsd:date ;
    rdfs:isDefinedBy sector-law: ;
    sw:term_status "accepted"@en ;
    skos:broader sector-law:CrimeVictimSafetyManagement ;
    skos:definition "Purposes associated with safety assessment of victims of criminal activities within the legal system"@en ;
    skos:inScheme sector-law:purposes-classes ;
    skos:prefLabel "Crime Victim Safety Assessment"@en .

sector-law:CrimeVictimSafetyManagement a rdfs:Class,
        skos:Concept,
        dpv:Purpose ;
    dct:created "2024-12-01"^^xsd:date ;
    rdfs:isDefinedBy sector-law: ;
    sw:term_status "accepted"@en ;
    skos:broader sector-law:CriminalLawEnforcement ;
    skos:definition "Purposes associated with management of safety for victims of criminal activities within the legal system"@en ;
    skos:inScheme sector-law:purposes-classes ;
    skos:prefLabel "Crime Victim Safety Management"@en .

sector-law:CrimeVictimSafetyProvision a rdfs:Class,
        skos:Concept,
        dpv:Purpose ;
    dct:created "2024-12-01"^^xsd:date ;
    rdfs:isDefinedBy sector-law: ;
    sw:term_status "accepted"@en ;
    skos:broader sector-law:CrimeVictimSafetyManagement ;
    skos:definition "Purposes associated with managing and providing safety for victims of criminal activities within the legal system"@en ;
    skos:inScheme sector-law:purposes-classes ;
    skos:prefLabel "Crime Victim Safety Provision"@en .

sector-law:CriminalBehaviourDetection a rdfs:Class,
        skos:Concept,
        dpv:Purpose ;
    dct:created "2024-12-01"^^xsd:date ;
    rdfs:isDefinedBy sector-law: ;
    sw:term_status "accepted"@en ;
    skos:broader sector-law:CrimeDetection ;
    skos:definition "Purposes associated with detection of criminal behaviour within the legal system"@en ;
    skos:inScheme sector-law:purposes-classes ;
    skos:prefLabel "Criminal Behaviour Detection"@en .

sector-law:CriminalLawEnforcement a rdfs:Class,
        skos:Concept,
        dpv:Purpose ;
    dct:created "2024-12-01"^^xsd:date ;
    rdfs:isDefinedBy sector-law: ;
    sw:term_status "accepted"@en ;
    skos:broader sector-law:LawEnforcement ;
    skos:definition "Purposes associated with criminal law enforcement within the legal system"@en ;
    skos:inScheme sector-law:purposes-classes ;
    skos:prefLabel "Criminal Law Enforcement"@en .

sector-law:ImmigrationApplicationAssessment a rdfs:Class,
        skos:Concept,
        dpv:Purpose ;
    dct:created "2024-12-01"^^xsd:date ;
    rdfs:isDefinedBy sector-law: ;
    sw:term_status "accepted"@en ;
    skos:broader sector-law:ImmigrationApplicationManagement ;
    skos:definition "Purposes associated with assessment of applications for validity, determination of outcomes such as visa durations, and determining decisions such as visa approved related to immigration within the legal system"@en ;
    skos:inScheme sector-law:purposes-classes ;
    skos:prefLabel "Immigration Application Assessment"@en .

sector-law:ImmigrationApplicationCollection a rdfs:Class,
        skos:Concept,
        dpv:Purpose ;
    dct:created "2024-12-01"^^xsd:date ;
    rdfs:isDefinedBy sector-law: ;
    sw:term_status "accepted"@en ;
    skos:broader sector-law:ImmigrationApplicationManagement ;
    skos:definition "xPurposes associated with collection of applications related to immigration within the legal system"@en ;
    skos:inScheme sector-law:purposes-classes ;
    skos:prefLabel "Immigration Application Collection"@en .

sector-law:ImmigrationApplicationManagement a rdfs:Class,
        skos:Concept,
        dpv:Purpose ;
    dct:created "2024-12-01"^^xsd:date ;
    rdfs:isDefinedBy sector-law: ;
    sw:term_status "accepted"@en ;
    skos:broader sector-law:ImmigrationRequestManagement ;
    skos:definition "Purposes associated with management of applications related to immigration within the legal system"@en ;
    skos:inScheme sector-law:purposes-classes ;
    skos:prefLabel "Immigration Application Management"@en .

sector-law:ImmigrationApplicationScreening a rdfs:Class,
        skos:Concept,
        dpv:Purpose ;
    dct:created "2024-12-01"^^xsd:date ;
    rdfs:isDefinedBy sector-law: ;
    sw:term_status "accepted"@en ;
    skos:broader sector-law:ImmigrationApplicationManagement ;
    skos:definition "Purposes associated with screening or filtering applications related to immigration within the legal system"@en ;
    skos:inScheme sector-law:purposes-classes ;
    skos:prefLabel "Immigration Application Screening"@en .

sector-law:ImmigrationAsylumManagement a rdfs:Class,
        skos:Concept,
        dpv:Purpose ;
    dct:created "2024-12-01"^^xsd:date ;
    rdfs:isDefinedBy sector-law: ;
    sw:term_status "accepted"@en ;
    skos:broader sector-law:ImmigrationManagement ;
    skos:definition "Purposes associated with management of requests or petitions for asylum including collecting and processing of applications, determining elibility, making and communicating decisions, and enforcing the limits as related to immigration within the legal system"@en ;
    skos:inScheme sector-law:purposes-classes ;
    skos:prefLabel "Immigration Asylum Management"@en .

sector-law:ImmigrationBorderControlManagement a rdfs:Class,
        skos:Concept,
        dpv:Purpose ;
    dct:created "2024-12-01"^^xsd:date ;
    rdfs:isDefinedBy sector-law: ;
    sw:term_status "accepted"@en ;
    skos:broader sector-law:ImmigrationSecurityManagement ;
    skos:definition "Purposes associated with border control within the legal system"@en ;
    skos:inScheme sector-law:purposes-classes ;
    skos:prefLabel "Immigration Border Control Management"@en .

sector-law:ImmigrationBorderDocumentVerification a rdfs:Class,
        skos:Concept,
        dpv:Purpose ;
    dct:created "2024-12-01"^^xsd:date ;
    rdfs:isDefinedBy sector-law: ;
    sw:term_status "accepted"@en ;
    skos:broader sector-law:ImmigrationBorderControlManagement ;
    skos:definition "Purposes associated with verification of documents and information at the border as defined in the legal system"@en ;
    skos:inScheme sector-law:purposes-classes ;
    skos:prefLabel "Immigration Border Document Verification"@en .

sector-law:ImmigrationBorderIdentityVerification a rdfs:Class,
        skos:Concept,
        dpv:Purpose ;
    dct:created "2024-12-01"^^xsd:date ;
    rdfs:isDefinedBy sector-law: ;
    sw:term_status "accepted"@en ;
    skos:broader sector-law:ImmigrationBorderControlManagement ;
    skos:definition "Purposes associated with verification of identity at the border as defined in the legal system"@en ;
    skos:inScheme sector-law:purposes-classes ;
    skos:prefLabel "Immigration Border Identity Verification"@en .

sector-law:ImmigrationClaimVerification a rdfs:Class,
        skos:Concept,
        dpv:Purpose ;
    dct:created "2024-12-01"^^xsd:date ;
    rdfs:isDefinedBy sector-law: ;
    sw:term_status "accepted"@en ;
    skos:broader sector-law:ImmigrationRequestManagement ;
    skos:definition "Purposes associated with verification of claims, such as background, history, and past life related to immigration within the legal system"@en ;
    skos:inScheme sector-law:purposes-classes ;
    skos:prefLabel "Immigration Claim Verification"@en .

sector-law:ImmigrationComplaintManagement a rdfs:Class,
        skos:Concept,
        dpv:Purpose ;
    dct:created "2024-12-01"^^xsd:date ;
    rdfs:isDefinedBy sector-law: ;
    sw:term_status "accepted"@en ;
    skos:broader sector-law:ImmigrationManagement ;
    skos:definition "Purposes associated with management of complaints related to immigration within the legal system"@en ;
    skos:inScheme sector-law:purposes-classes ;
    skos:prefLabel "Immigration Complaint Management"@en .

sector-law:ImmigrationDecisionCommunication a rdfs:Class,
        skos:Concept,
        dpv:Purpose ;
    dct:created "2024-12-01"^^xsd:date ;
    rdfs:isDefinedBy sector-law: ;
    sw:term_status "accepted"@en ;
    skos:broader sector-law:ImmigrationRequestManagement ;
    skos:definition "Purposes associated with communicating decisions for applications related to immigration within the legal system"@en ;
    skos:inScheme sector-law:purposes-classes ;
    skos:prefLabel "Immigration Decision Communication"@en .

sector-law:ImmigrationDocumentVerficiation a rdfs:Class,
        skos:Concept,
        dpv:Purpose ;
    dct:created "2024-12-01"^^xsd:date ;
    rdfs:isDefinedBy sector-law: ;
    sw:term_status "accepted"@en ;
    skos:broader sector-law:ImmigrationRequestManagement ;
    skos:definition "Purposes associated with verification of documents and information related to immigration within the legal system"@en ;
    skos:inScheme sector-law:purposes-classes ;
    skos:prefLabel "Immigration Document Verficiation"@en .

sector-law:ImmigrationEligibilityAssessment a rdfs:Class,
        skos:Concept,
        dpv:Purpose ;
    dct:created "2024-12-01"^^xsd:date ;
    rdfs:isDefinedBy sector-law: ;
    sw:term_status "accepted"@en ;
    skos:broader sector-law:ImmigrationRequestManagement ;
    skos:definition "Purposes associated with assessment of eligibility related to immigration within the legal system"@en ;
    skos:inScheme sector-law:purposes-classes ;
    skos:prefLabel "Immigration Eligibility Assessment"@en .

sector-law:ImmigrationExpiredPermitManagement a rdfs:Class,
        skos:Concept,
        dpv:Purpose ;
    dct:created "2024-12-01"^^xsd:date ;
    rdfs:isDefinedBy sector-law: ;
    sw:term_status "accepted"@en ;
    skos:broader sector-law:ImmigrationSecurityManagement ;
    skos:definition "Purposes associated with management of expired visas, authorisations, and other permits related to immigration within the legal system"@en ;
    skos:inScheme sector-law:purposes-classes ;
    skos:prefLabel "Immigration Expired Permit Management"@en .

sector-law:ImmigrationFraudManagement a rdfs:Class,
        skos:Concept,
        dpv:Purpose ;
    dct:created "2024-12-01"^^xsd:date ;
    rdfs:isDefinedBy sector-law: ;
    sw:term_status "accepted"@en ;
    skos:broader sector-law:ImmigrationSecurityManagement ;
    skos:definition "Purposes associated with detection and prevention of fraud related to immigration within the legal system"@en ;
    skos:inScheme sector-law:purposes-classes ;
    skos:prefLabel "Immigration Fraud Management"@en .

sector-law:ImmigrationHealthRiskDetection a rdfs:Class,
        skos:Concept,
        dpv:Purpose ;
    dct:created "2024-12-01"^^xsd:date ;
    rdfs:isDefinedBy sector-law: ;
    sw:term_status "accepted"@en ;
    skos:broader sector-law:ImmigrationHealthRiskManagement ;
    skos:definition "Purposes related to detecting health risks as part of security related to immigration within the legal system"@en ;
    skos:inScheme sector-law:purposes-classes ;
    skos:prefLabel "Immigration Health Risk Detection"@en .

sector-law:ImmigrationHealthRiskManagement a rdfs:Class,
        skos:Concept,
        dpv:Purpose ;
    dct:created "2024-12-01"^^xsd:date ;
    rdfs:isDefinedBy sector-law: ;
    sw:term_status "accepted"@en ;
    skos:broader sector-law:ImmigrationSecurityManagement ;
    skos:definition "Purposes related to management of health risks as part of security related to immigration within the legal system"@en ;
    skos:inScheme sector-law:purposes-classes ;
    skos:prefLabel "Immigration Health Risk Management"@en .

sector-law:ImmigrationHealthRiskPrediction a rdfs:Class,
        skos:Concept,
        dpv:Purpose ;
    dct:created "2024-12-01"^^xsd:date ;
    rdfs:isDefinedBy sector-law: ;
    sw:term_status "accepted"@en ;
    skos:broader sector-law:ImmigrationHealthRiskManagement ;
    skos:definition "Purposes related to predicting health risks as part of security related to immigration within the legal system"@en ;
    skos:inScheme sector-law:purposes-classes ;
    skos:prefLabel "Immigration Health Risk Prediction"@en .

sector-law:ImmigrationIdentityVerification a rdfs:Class,
        skos:Concept,
        dpv:Purpose ;
    dct:created "2024-12-01"^^xsd:date ;
    rdfs:isDefinedBy sector-law: ;
    sw:term_status "accepted"@en ;
    skos:broader dpv:IdentityVerification,
        sector-law:ImmigrationRequestManagement ;
    skos:definition "Purposes associated with verificiation of identity related to immigration within the legal system"@en ;
    skos:inScheme sector-law:purposes-classes ;
    skos:prefLabel "Immigration Identity Verification"@en .

sector-law:ImmigrationManagement a rdfs:Class,
        skos:Concept,
        dpv:Purpose ;
    dct:created "2024-12-01"^^xsd:date ;
    rdfs:isDefinedBy sector-law: ;
    sw:term_status "accepted"@en ;
    skos:broader sector-law:JusticeManagement ;
    skos:definition "Purposes associated with management of immigration within the legal system"@en ;
    skos:inScheme sector-law:purposes-classes ;
    skos:prefLabel "Immigration Management"@en .

sector-law:ImmigrationMigrationManagement a rdfs:Class,
        skos:Concept,
        dpv:Purpose ;
    dct:created "2024-12-01"^^xsd:date ;
    rdfs:isDefinedBy sector-law: ;
    sw:term_status "accepted"@en ;
    skos:broader sector-law:ImmigrationManagement ;
    skos:definition "Purposes associated with management of requests or petitions for migration including collecting and processing of applications, determining elibility, making and communicating decisions, and enforcing the limits as related to immigration within the legal system"@en ;
    skos:inScheme sector-law:purposes-classes ;
    skos:prefLabel "Immigration Migration Management"@en .

sector-law:ImmigrationRequestManagement a rdfs:Class,
        skos:Concept,
        dpv:Purpose ;
    dct:created "2024-12-01"^^xsd:date ;
    rdfs:isDefinedBy sector-law: ;
    sw:term_status "accepted"@en ;
    skos:broader sector-law:ImmigrationManagement ;
    skos:definition "Purposes associated with management of requests related to immigration within the legal system"@en ;
    skos:inScheme sector-law:purposes-classes ;
    skos:prefLabel "Immigration Request Management"@en .

sector-law:ImmigrationResidencyPermitManagement a rdfs:Class,
        skos:Concept,
        dpv:Purpose ;
    dct:created "2024-12-01"^^xsd:date ;
    rdfs:isDefinedBy sector-law: ;
    sw:term_status "accepted"@en ;
    skos:broader sector-law:ImmigrationManagement ;
    skos:definition "Purposes associated with management of residency permits, including collecting and processing of applications, determining elibility, making and communicating decisions, and enforcing the limits as related to immigration within the legal system"@en ;
    skos:inScheme sector-law:purposes-classes ;
    skos:prefLabel "Immigration Residency Permit Management"@en .

sector-law:ImmigrationSecurityManagement a rdfs:Class,
        skos:Concept,
        dpv:Purpose ;
    dct:created "2024-12-01"^^xsd:date ;
    rdfs:isDefinedBy sector-law: ;
    sw:term_status "accepted"@en ;
    skos:broader sector-law:ImmigrationManagement ;
    skos:definition "Purposes related to management of security related to immigration within the legal system"@en ;
    skos:inScheme sector-law:purposes-classes ;
    skos:prefLabel "Immigration Security Management"@en .

sector-law:ImmigrationTransitPermitManagement a rdfs:Class,
        skos:Concept,
        dpv:Purpose ;
    dct:created "2024-12-01"^^xsd:date ;
    rdfs:isDefinedBy sector-law: ;
    sw:term_status "accepted"@en ;
    skos:broader sector-law:ImmigrationManagement ;
    skos:definition "Purposes associated with management of transit permits or transit visas, including collecting and processing of applications, determining elibility, making and communicating decisions, and enforcing the limits as related to immigration within the legal system"@en ;
    skos:inScheme sector-law:purposes-classes ;
    skos:prefLabel "Immigration Transit Permit Management"@en .

sector-law:ImmigrationVisaManagement a rdfs:Class,
        skos:Concept,
        dpv:Purpose ;
    dct:created "2024-12-01"^^xsd:date ;
    rdfs:isDefinedBy sector-law: ;
    sw:term_status "accepted"@en ;
    skos:broader sector-law:ImmigrationManagement ;
    skos:definition "Purposes associated with management of visas, including collecting and processing of applications, determining elibility, making and communicating decisions, and enforcing the limits as related to immigration within the legal system"@en ;
    skos:inScheme sector-law:purposes-classes ;
    skos:prefLabel "Immigration Visa Management"@en .

sector-law:ImmigrationWorkAuthorisationManagement a rdfs:Class,
        skos:Concept,
        dpv:Purpose ;
    dct:created "2024-12-01"^^xsd:date ;
    rdfs:isDefinedBy sector-law: ;
    sw:term_status "accepted"@en ;
    skos:broader sector-law:ImmigrationManagement ;
    skos:definition "Purposes associated with management of work authorisations, including collecting and processing of applications, determining elibility, making and communicating decisions, and enforcing the limits as related to immigration within the legal system"@en ;
    skos:inScheme sector-law:purposes-classes ;
    skos:prefLabel "Immigration Work Authorisation Management"@en .

sector-law:JudicialCaseManagement a rdfs:Class,
        skos:Concept,
        dpv:Purpose ;
    dct:created "2024-12-01"^^xsd:date ;
    rdfs:isDefinedBy sector-law: ;
    sw:term_status "accepted"@en ;
    skos:broader sector-law:JudicialSystemManagement ;
    skos:definition "Purposes associated with management of cases within the judicial system"@en ;
    skos:inScheme sector-law:purposes-classes ;
    skos:prefLabel "Judicial Case Management"@en .

sector-law:JudicialDecisionMaking a rdfs:Class,
        skos:Concept,
        dpv:Purpose ;
    dct:created "2024-12-01"^^xsd:date ;
    rdfs:isDefinedBy sector-law: ;
    sw:term_status "accepted"@en ;
    skos:broader sector-law:JudicialSystemManagement ;
    skos:definition "Purposes associated with making decisions related to legal determinations within the judicial system such as in courts cases or in authority rulings"@en ;
    skos:inScheme sector-law:purposes-classes ;
    skos:prefLabel "Judicial Decision Making"@en .

sector-law:JudicialDisputeManagement a rdfs:Class,
        skos:Concept,
        dpv:Purpose ;
    dct:created "2024-12-01"^^xsd:date ;
    rdfs:isDefinedBy sector-law: ;
    sw:term_status "accepted"@en ;
    skos:broader sector-law:JudicialSystemManagement ;
    skos:definition "Purposes associated with detection, assessment, identifying resolutions, and other activities related to management of disputes within the judicial system"@en ;
    skos:inScheme sector-law:purposes-classes ;
    skos:prefLabel "Judicial Dispute Management"@en .

sector-law:JudicialLegalInterpretation a rdfs:Class,
        skos:Concept,
        dpv:Purpose ;
    dct:created "2024-12-01"^^xsd:date ;
    rdfs:isDefinedBy sector-law: ;
    sw:term_status "accepted"@en ;
    skos:broader sector-law:JudicialSystemManagement ;
    skos:definition "Purposes associated with interpretation of laws, arguments, and facts and other related information within the judicial system"@en ;
    skos:inScheme sector-law:purposes-classes ;
    skos:prefLabel "Judicial Legal Interpretation"@en .

sector-law:JudicialRecordKeeping a rdfs:Class,
        skos:Concept,
        dpv:Purpose ;
    dct:created "2024-12-01"^^xsd:date ;
    rdfs:isDefinedBy sector-law: ;
    sw:term_status "accepted"@en ;
    skos:broader sector-law:JudicialSystemManagement ;
    skos:definition "Purposes associated with record keeping within the judicial system"@en ;
    skos:inScheme sector-law:purposes-classes ;
    skos:prefLabel "Judicial Record Keeping"@en .

sector-law:JudicialSystemManagement a rdfs:Class,
        skos:Concept,
        dpv:Purpose ;
    dct:created "2024-12-01"^^xsd:date ;
    rdfs:isDefinedBy sector-law: ;
    sw:term_status "accepted"@en ;
    skos:broader sector-law:JusticeManagement ;
    skos:definition "Purposes associated with administration and coordination of the operations, processes, and resources within the judicial system"@en ;
    skos:inScheme sector-law:purposes-classes ;
    skos:prefLabel "Judicial System Management"@en .

sector-law:JusticeManagement a rdfs:Class,
        skos:Concept,
        dpv:Purpose ;
    dct:created "2024-12-01"^^xsd:date ;
    rdfs:isDefinedBy sector-law: ;
    sw:term_status "accepted"@en ;
    skos:broader dpv:Purpose ;
    skos:definition "Purposes associated with administration of justice within the legal system"@en ;
    skos:inScheme sector-law:purposes-classes ;
    skos:prefLabel "Justice Management"@en .

sector-law:LawEnforcement a rdfs:Class,
        skos:Concept,
        dpv:Purpose ;
    dct:created "2024-12-01"^^xsd:date ;
    rdfs:isDefinedBy sector-law: ;
    sw:term_status "accepted"@en ;
    skos:broader sector-law:JusticeManagement ;
    skos:definition "Purposes associated with law enforcement within the legal system"@en ;
    skos:inScheme sector-law:purposes-classes ;
    skos:prefLabel "Law Enforcement"@en .

sector-law:LegalAidProvision a rdfs:Class,
        skos:Concept,
        dpv:Purpose ;
    dct:created "2024-12-01"^^xsd:date ;
    rdfs:isDefinedBy sector-law: ;
    sw:term_status "accepted"@en ;
    skos:broader sector-law:JudicialSystemManagement ;
    skos:definition "Purposes associated with provision of legal aid within the judicial system"@en ;
    skos:inScheme sector-law:purposes-classes ;
    skos:prefLabel "Legal Aid Provision"@en .

sector-law:LegalComplaintManagement a rdfs:Class,
        skos:Concept,
        dpv:Purpose ;
    dct:created "2024-12-01"^^xsd:date ;
    rdfs:isDefinedBy sector-law: ;
    sw:term_status "accepted"@en ;
    skos:broader sector-law:JudicialSystemManagement ;
    skos:definition "Purposes associated with management of complaints within the judicial system"@en ;
    skos:inScheme sector-law:purposes-classes ;
    skos:prefLabel "Legal Complaint Management"@en .

sector-law:LegalEvidenceCollection a rdfs:Class,
        skos:Concept,
        dpv:Purpose ;
    dct:created "2024-12-01"^^xsd:date ;
    rdfs:isDefinedBy sector-law: ;
    sw:term_status "accepted"@en ;
    skos:broader sector-law:LegalInvestigation ;
    skos:definition "Purposes associated with collection and management of evidence for investigation within the legal system"@en ;
    skos:inScheme sector-law:purposes-classes ;
    skos:prefLabel "Legal Evidence Collection"@en .

sector-law:LegalEvidenceEligibilityAssessment a rdfs:Class,
        skos:Concept,
        dpv:Purpose ;
    dct:created "2024-12-01"^^xsd:date ;
    rdfs:isDefinedBy sector-law: ;
    sw:term_status "accepted"@en ;
    skos:broader sector-law:LegalInvestigation ;
    skos:definition "Purposes associated with the assessment of eligibility of evidence for investigation within the legal system"@en ;
    skos:inScheme sector-law:purposes-classes ;
    skos:prefLabel "Legal Evidence Eligibility Assessment"@en .

sector-law:LegalEvidenceInterpretation a rdfs:Class,
        skos:Concept,
        dpv:Purpose ;
    dct:created "2024-12-01"^^xsd:date ;
    rdfs:isDefinedBy sector-law: ;
    sw:term_status "accepted"@en ;
    skos:broader sector-law:LegalInvestigation ;
    skos:definition "Purposes associated with interpretation of evidence for investigation within the legal system"@en ;
    skos:inScheme sector-law:purposes-classes ;
    skos:prefLabel "Legal Evidence Interpretation"@en .

sector-law:LegalFirstOffencePrediction a rdfs:Class,
        skos:Concept,
        dpv:Purpose ;
    dct:created "2024-12-01"^^xsd:date ;
    rdfs:isDefinedBy sector-law: ;
    sw:term_status "accepted"@en ;
    skos:broader sector-law:LegalOffencePrediction ;
    skos:definition "Purposes associated with predicting the first occurence related to offences, violations, crime, or other activities of interest within the legal system"@en ;
    skos:inScheme sector-law:purposes-classes ;
    skos:prefLabel "Legal First Offence Prediction"@en .

sector-law:LegalInstitutionalManagement a rdfs:Class,
        skos:Concept,
        dpv:Purpose ;
    dct:created "2024-12-01"^^xsd:date ;
    rdfs:isDefinedBy sector-law: ;
    sw:term_status "accepted"@en ;
    skos:broader sector-law:JusticeManagement ;
    skos:definition "Purposes associated with management of institutions part of the legal system"@en ;
    skos:inScheme sector-law:purposes-classes ;
    skos:prefLabel "Legal Institutional Management"@en .

sector-law:LegalInterrogation a rdfs:Class,
        skos:Concept,
        dpv:Purpose ;
    dct:created "2024-12-01"^^xsd:date ;
    rdfs:isDefinedBy sector-law: ;
    sw:term_status "accepted"@en ;
    skos:broader sector-law:LegalInvestigation ;
    skos:definition "Purposes associated with questioning of individuals in relation to an investigation or other matters within the legal system"@en ;
    skos:inScheme sector-law:purposes-classes ;
    skos:prefLabel "Legal Interrogation"@en .

sector-law:LegalInvestigation a rdfs:Class,
        skos:Concept,
        dpv:Purpose ;
    dct:created "2024-12-01"^^xsd:date ;
    rdfs:isDefinedBy sector-law: ;
    sw:term_status "accepted"@en ;
    skos:broader sector-law:LawEnforcement ;
    skos:definition "Purposes associated with investigations within the legal system"@en ;
    skos:inScheme sector-law:purposes-classes ;
    skos:prefLabel "Legal Investigation"@en .

sector-law:LegalOffenceDetection a rdfs:Class,
        skos:Concept,
        dpv:Purpose ;
    dct:created "2024-12-01"^^xsd:date ;
    rdfs:isDefinedBy sector-law: ;
    sw:term_status "accepted"@en ;
    skos:broader sector-law:LawEnforcement ;
    skos:definition "Purposes associated with identifying or discovering illegal activities or violations or offences within the legal system"@en ;
    skos:inScheme sector-law:purposes-classes ;
    skos:prefLabel "Legal Offence Detection"@en .

sector-law:LegalOffencePatternAnalysis a rdfs:Class,
        skos:Concept,
        dpv:Purpose ;
    dct:created "2024-12-01"^^xsd:date ;
    rdfs:isDefinedBy sector-law: ;
    sw:term_status "accepted"@en ;
    skos:broader sector-law:LegalResearchDevelopment ;
    skos:definition "Purposes associated with identifying and analysing patterns and trends related to offences, violations, crime, or other activities of interest within the legal system"@en ;
    skos:inScheme sector-law:purposes-classes ;
    skos:prefLabel "Legal Offence Pattern Analysis"@en .

sector-law:LegalOffencePrediction a rdfs:Class,
        skos:Concept,
        dpv:Purpose ;
    dct:created "2024-12-01"^^xsd:date ;
    rdfs:isDefinedBy sector-law: ;
    sw:term_status "accepted"@en ;
    skos:broader sector-law:LegalResearchDevelopment ;
    skos:definition "Purposes associated with predicting occurences or patterns related to offences, violations, crime, or other activities of interest within the legal system"@en ;
    skos:inScheme sector-law:purposes-classes ;
    skos:prefLabel "Legal Offence Prediction"@en .

sector-law:LegalOffenceProsecution a rdfs:Class,
        skos:Concept,
        dpv:Purpose ;
    dct:created "2024-12-01"^^xsd:date ;
    rdfs:isDefinedBy sector-law: ;
    sw:term_status "accepted"@en ;
    skos:broader sector-law:LawEnforcement ;
    skos:definition "Purposes associated with prosecution of illegal activities or violations or offences within the legal system"@en ;
    skos:inScheme sector-law:purposes-classes ;
    skos:prefLabel "Legal Offence Prosecution"@en .

sector-law:LegalOffenceSurveillance a rdfs:Class,
        skos:Concept,
        dpv:Purpose ;
    dct:created "2024-12-01"^^xsd:date ;
    rdfs:isDefinedBy sector-law: ;
    sw:term_status "accepted"@en ;
    skos:broader sector-law:LawEnforcement ;
    skos:definition "Purposes associated with monitoring or observing to detect or deter potential or ongoing illegal activities or violations or offences within the legal system"@en ;
    skos:inScheme sector-law:purposes-classes ;
    skos:prefLabel "Legal Offence Surveillance"@en .

sector-law:LegalRepeatOffencePrediction a rdfs:Class,
        skos:Concept,
        dpv:Purpose ;
    dct:created "2024-12-01"^^xsd:date ;
    rdfs:isDefinedBy sector-law: ;
    sw:term_status "accepted"@en ;
    skos:broader sector-law:LegalOffencePrediction ;
    skos:definition "Purposes associated with predicting the subsequent or repeated occurences related to offences, violations, crime, or other activities of interest within the legal system"@en ;
    skos:inScheme sector-law:purposes-classes ;
    skos:prefLabel "Legal Repeat Offence Prediction"@en .

sector-law:LegalResearchDevelopment a rdfs:Class,
        skos:Concept,
        dpv:Purpose ;
    dct:created "2024-12-01"^^xsd:date ;
    rdfs:isDefinedBy sector-law: ;
    sw:term_status "accepted"@en ;
    skos:broader sector-law:LawEnforcement ;
    skos:definition "Purposes associated with research and development within the legal system"@en ;
    skos:inScheme sector-law:purposes-classes ;
    skos:prefLabel "Legal Research Development"@en .

sector-law:LegalSuspectedOffenceInvestigation a rdfs:Class,
        skos:Concept,
        dpv:Purpose ;
    dct:created "2024-12-01"^^xsd:date ;
    rdfs:isDefinedBy sector-law: ;
    sw:term_status "accepted"@en ;
    skos:broader sector-law:LegalInvestigation ;
    skos:definition "Purposes associated with investigation of suspected offences, violations, crime, or other activities of interest within the legal system"@en ;
    skos:inScheme sector-law:purposes-classes ;
    skos:prefLabel "Legal Suspected Offence Investigation"@en .

sector-law:PrisonManagement a rdfs:Class,
        skos:Concept,
        dpv:Purpose ;
    dct:created "2024-12-01"^^xsd:date ;
    rdfs:isDefinedBy sector-law: ;
    sw:term_status "accepted"@en ;
    skos:broader sector-law:LegalInstitutionalManagement ;
    skos:definition "Purposes associated with management of prison institutions part of the legal system"@en ;
    skos:inScheme sector-law:purposes-classes ;
    skos:prefLabel "Prison Management"@en .

sector-law:ProbationManagement a rdfs:Class,
        skos:Concept,
        dpv:Purpose ;
    dct:created "2024-12-01"^^xsd:date ;
    rdfs:isDefinedBy sector-law: ;
    sw:term_status "accepted"@en ;
    skos:broader sector-law:LegalInstitutionalManagement ;
    skos:definition "Purposes associated with management of probation institutions part of the legal system"@en ;
    skos:inScheme sector-law:purposes-classes ;
    skos:prefLabel "Probation Management"@en .

sector-law:PublicTransportFraudManagement a rdfs:Class,
        skos:Concept,
        dpv:Purpose ;
    dct:created "2024-12-01"^^xsd:date ;
    rdfs:isDefinedBy sector-law: ;
    sw:term_status "accepted"@en ;
    skos:broader sector-law:PublicTransportLawEnforcement ;
    skos:definition "Purposes associated with fraud prevention and detection and management related to public transport infrastructure and services"@en ;
    skos:inScheme sector-law:purposes-classes ;
    skos:prefLabel "Public Transport Fraud Management"@en .

sector-law:PublicTransportLawEnforcement a rdfs:Class,
        skos:Concept,
        dpv:Purpose ;
    dct:created "2024-12-01"^^xsd:date ;
    rdfs:isDefinedBy sector-law: ;
    sw:term_status "accepted"@en ;
    skos:broader sector-law:RoadTrafficLawEnforcement ;
    skos:definition "Purposes associated with enforcement of road traffic law for public transport infrastructure and services"@en ;
    skos:inScheme sector-law:purposes-classes ;
    skos:prefLabel "Public Transport Law Enforcement"@en .

sector-law:PublicTransportSafetyMonitoring a rdfs:Class,
        skos:Concept,
        dpv:Purpose ;
    dct:created "2024-12-01"^^xsd:date ;
    rdfs:isDefinedBy sector-law: ;
    sw:term_status "accepted"@en ;
    skos:broader sector-law:PublicTransportLawEnforcement ;
    skos:definition "Purposes associated with monitoring public transport infrastructure and services for the purposes of public safety"@en ;
    skos:inScheme sector-law:purposes-classes ;
    skos:prefLabel "Public Transport Safety Monitoring"@en .

sector-law:PublicTransportViolationDetection a rdfs:Class,
        skos:Concept,
        dpv:Purpose ;
    dct:created "2024-12-01"^^xsd:date ;
    rdfs:isDefinedBy sector-law: ;
    sw:term_status "accepted"@en ;
    skos:broader sector-law:PublicTransportLawEnforcement ;
    skos:definition "Purposes associated with detection of violations  related to road traffic law within or including public transport"@en ;
    skos:inScheme sector-law:purposes-classes ;
    skos:prefLabel "Public Transport Violation Detection"@en .

sector-law:RecidivismPrediction a rdfs:Class,
        skos:Concept,
        dpv:Purpose ;
    dct:created "2024-12-01"^^xsd:date ;
    rdfs:isDefinedBy sector-law: ;
    sw:term_status "accepted"@en ;
    skos:broader sector-law:LegalRepeatOffencePrediction ;
    skos:definition "Purposes associated with prediction of recidivism as the repeating of an undesirable behaviours or offences or violations by an entity after they have experienced negative consequences of that behaviour or have been informed or trained on how to avoid repeating it"@en ;
    skos:inScheme sector-law:purposes-classes ;
    skos:prefLabel "Recidivism Prediction"@en .

sector-law:RehabilitationManagement a rdfs:Class,
        skos:Concept,
        dpv:Purpose ;
    dct:created "2024-12-01"^^xsd:date ;
    rdfs:isDefinedBy sector-law: ;
    sw:term_status "accepted"@en ;
    skos:broader sector-law:LegalInstitutionalManagement ;
    skos:definition "Purposes associated with management of rehabilitation institutions part of the legal system"@en ;
    skos:inScheme sector-law:purposes-classes ;
    skos:prefLabel "Rehabilitation Management"@en .

sector-law:RoadDUIEnforcement a rdfs:Class,
        skos:Concept,
        dpv:Purpose ;
    dct:created "2024-12-01"^^xsd:date ;
    rdfs:isDefinedBy sector-law: ;
    sw:term_status "accepted"@en ;
    skos:broader sector-law:RoadTrafficRuleEnforcement ;
    skos:definition "Purposes associated with detection and enforcement of DUI (driving under influence) rules on roads"@en ;
    skos:inScheme sector-law:purposes-classes ;
    skos:prefLabel "Road DUIEnforcement"@en .

sector-law:RoadParkingEnforcement a rdfs:Class,
        skos:Concept,
        dpv:Purpose ;
    dct:created "2024-12-01"^^xsd:date ;
    rdfs:isDefinedBy sector-law: ;
    sw:term_status "accepted"@en ;
    skos:broader sector-law:RoadTrafficRuleEnforcement ;
    skos:definition "Purposes associated with detection and enforcement of parking rules on roads"@en ;
    skos:inScheme sector-law:purposes-classes ;
    skos:prefLabel "Road Parking Enforcement"@en .

sector-law:RoadSpeedLimitEnforcement a rdfs:Class,
        skos:Concept,
        dpv:Purpose ;
    dct:created "2024-12-01"^^xsd:date ;
    rdfs:isDefinedBy sector-law: ;
    sw:term_status "accepted"@en ;
    skos:broader sector-law:RoadTrafficRuleEnforcement ;
    skos:definition "Purposes associated with detection and enforcement of speed limits on roads"@en ;
    skos:inScheme sector-law:purposes-classes ;
    skos:prefLabel "Road Speed Limit Enforcement"@en .

sector-law:RoadTollViolationDetection a rdfs:Class,
        skos:Concept,
        dpv:Purpose ;
    dct:created "2024-12-01"^^xsd:date ;
    rdfs:isDefinedBy sector-law: ;
    sw:term_status "accepted"@en ;
    skos:broader sector-infra:RoadTollManagement,
        sector-law:RoadTrafficLawEnforcement ;
    skos:definition "Purposes associated with detection of violations related to road toll collection and payment"@en ;
    skos:inScheme sector-law:purposes-classes ;
    skos:prefLabel "Road Toll Violation Detection"@en .

sector-law:RoadTrafficLawEnforcement a rdfs:Class,
        skos:Concept,
        dpv:Purpose ;
    dct:created "2024-12-01"^^xsd:date ;
    rdfs:isDefinedBy sector-law: ;
    sw:term_status "accepted"@en ;
    skos:broader sector-law:TransportLawEnforcement ;
    skos:definition "Purposes associated with law enforcement related to road infrastructure and services"@en ;
    skos:inScheme sector-law:purposes-classes ;
    skos:prefLabel "Road Traffic Law Enforcement"@en .

sector-law:RoadTrafficLawViolationCommunication a rdfs:Class,
        skos:Concept,
        dpv:Purpose ;
    dct:created "2024-12-01"^^xsd:date ;
    rdfs:isDefinedBy sector-law: ;
    sw:term_status "accepted"@en ;
    skos:broader sector-law:RoadTrafficLawEnforcement ;
    skos:definition "Purposes associated with managing communications related to violations of road traffic law violations"@en ;
    skos:inScheme sector-law:purposes-classes ;
    skos:prefLabel "Road Traffic Law Violation Communication"@en .

sector-law:RoadTrafficLawViolationDetection a rdfs:Class,
        skos:Concept,
        dpv:Purpose ;
    dct:created "2024-12-01"^^xsd:date ;
    rdfs:isDefinedBy sector-law: ;
    sw:term_status "accepted"@en ;
    skos:broader sector-law:RoadTrafficLawEnforcement ;
    skos:definition "Purposes associated with detection of violations related to road traffic law"@en ;
    skos:inScheme sector-law:purposes-classes ;
    skos:prefLabel "Road Traffic Law Violation Detection"@en .

sector-law:RoadTrafficLawViolationFineAssessment a rdfs:Class,
        skos:Concept,
        dpv:Purpose ;
    dct:created "2024-12-01"^^xsd:date ;
    rdfs:isDefinedBy sector-law: ;
    sw:term_status "accepted"@en ;
    skos:broader sector-law:RoadTrafficLawEnforcement ;
    skos:definition "Purposes associated with determination and calculation related to assessment of fines for violaitions of road traffic law"@en ;
    skos:inScheme sector-law:purposes-classes ;
    skos:prefLabel "Road Traffic Law Violation Fine Assessment"@en .

sector-law:RoadTrafficLawViolationFineCollection a rdfs:Class,
        skos:Concept,
        dpv:Purpose ;
    dct:created "2024-12-01"^^xsd:date ;
    rdfs:isDefinedBy sector-law: ;
    sw:term_status "accepted"@en ;
    skos:broader sector-law:RoadTrafficLawEnforcement ;
    skos:definition "Purposes associated with managing payment and collection of fines related to violations of road traffic law"@en ;
    skos:inScheme sector-law:purposes-classes ;
    skos:prefLabel "Road Traffic Law Violation Fine Collection"@en .

sector-law:RoadTrafficRuleEnforcement a rdfs:Class,
        skos:Concept,
        dpv:Purpose ;
    dct:created "2024-12-01"^^xsd:date ;
    rdfs:isDefinedBy sector-law: ;
    sw:term_status "accepted"@en ;
    skos:broader sector-law:RoadTrafficLawEnforcement ;
    skos:definition "Purposes associated with detection and enforcement of traffic rules on roads"@en ;
    skos:inScheme sector-law:purposes-classes ;
    skos:prefLabel "Road Traffic Rule Enforcement"@en .

sector-law:RoadTrafficSignalEnforcement a rdfs:Class,
        skos:Concept,
        dpv:Purpose ;
    dct:created "2024-12-01"^^xsd:date ;
    rdfs:isDefinedBy sector-law: ;
    sw:term_status "accepted"@en ;
    skos:broader sector-law:RoadTrafficRuleEnforcement ;
    skos:definition "Purposes associated with detection and enforcement of traffic signals on roads"@en ;
    skos:inScheme sector-law:purposes-classes ;
    skos:prefLabel "Road Traffic Signal Enforcement"@en .

sector-law:RoadVehicleCertificationEnforcement a rdfs:Class,
        skos:Concept,
        dpv:Purpose ;
    dct:created "2024-12-01"^^xsd:date ;
    rdfs:isDefinedBy sector-law: ;
    sw:term_status "accepted"@en ;
    skos:broader sector-law:RoadTrafficLawEnforcement ;
    skos:definition "Purposes associated with detection and enforcement of road vehicle certifications"@en ;
    skos:inScheme sector-law:purposes-classes ;
    skos:prefLabel "Road Vehicle Certification Enforcement"@en .

sector-law:RoadVehicleEmissionEnforcement a rdfs:Class,
        skos:Concept,
        dpv:Purpose ;
    dct:created "2024-12-01"^^xsd:date ;
    rdfs:isDefinedBy sector-law: ;
    sw:term_status "accepted"@en ;
    skos:broader sector-law:RoadTrafficLawEnforcement ;
    skos:definition "Purposes associated with detection and enforcement of road vehicle emissions"@en ;
    skos:inScheme sector-law:purposes-classes ;
    skos:prefLabel "Road Vehicle Emission Enforcement"@en .

sector-law:RoadVehicleInsuranceEnforcement a rdfs:Class,
        skos:Concept,
        dpv:Purpose ;
    dct:created "2024-12-01"^^xsd:date ;
    rdfs:isDefinedBy sector-law: ;
    sw:term_status "accepted"@en ;
    skos:broader sector-law:RoadTrafficLawEnforcement ;
    skos:definition "Purposes associated with detection and enforcement of road vehicle insurance"@en ;
    skos:inScheme sector-law:purposes-classes ;
    skos:prefLabel "Road Vehicle Insurance Enforcement"@en .

sector-law:RoadVehicleRegistrationEnforcement a rdfs:Class,
        skos:Concept,
        dpv:Purpose ;
    dct:created "2024-12-01"^^xsd:date ;
    rdfs:isDefinedBy sector-law: ;
    sw:term_status "accepted"@en ;
    skos:broader sector-law:RoadTrafficLawEnforcement ;
    skos:definition "Purposes associated with detection and enforcement of road vehicle registration"@en ;
    skos:inScheme sector-law:purposes-classes ;
    skos:prefLabel "Road Vehicle Registration Enforcement"@en .

sector-law:SuspectedCrimeInvestigation a rdfs:Class,
        skos:Concept,
        dpv:Purpose ;
    dct:created "2024-12-01"^^xsd:date ;
    rdfs:isDefinedBy sector-law: ;
    sw:term_status "accepted"@en ;
    skos:broader sector-law:CriminalLawEnforcement,
        sector-law:LegalSuspectedOffenceInvestigation ;
    skos:definition "Purposes associated with investigation of suspected crimes within the legal system"@en ;
    skos:inScheme sector-law:purposes-classes ;
    skos:prefLabel "Suspected Crime Investigation"@en .

sector-law:SuspectedCriminalBehaviourDetection a rdfs:Class,
        skos:Concept,
        dpv:Purpose ;
    dct:created "2024-12-01"^^xsd:date ;
    rdfs:isDefinedBy sector-law: ;
    sw:term_status "accepted"@en ;
    skos:broader sector-law:CrimeDetection,
        sector-law:LegalSuspectedOffenceInvestigation ;
    skos:definition "Purposes associated with detection of suspected criminal behaviour within the legal system"@en ;
    skos:inScheme sector-law:purposes-classes ;
    skos:prefLabel "Suspected Criminal Behaviour Detection"@en .

sector-law:TransportLawEnforcement a rdfs:Class,
        skos:Concept,
        dpv:Purpose ;
    dct:created "2024-12-01"^^xsd:date ;
    rdfs:isDefinedBy sector-law: ;
    sw:term_status "accepted"@en ;
    skos:broader sector-law:LawEnforcement ;
    skos:definition "Purposes associated with law enforcement related to transportation infrastructure and services"@en ;
    skos:inScheme sector-law:purposes-classes ;
    skos:prefLabel "Transport Law Enforcement"@en .

sector-law:UnauthorisedMigrationDetection a rdfs:Class,
        skos:Concept,
        dpv:Purpose ;
    dct:created "2024-12-01"^^xsd:date ;
    rdfs:isDefinedBy sector-law: ;
    sw:term_status "accepted"@en ;
    skos:broader sector-law:UnauthorisedMigrationManagement ;
    skos:definition "Puposes associated with detecting unauthorised migration within the legal system"@en ;
    skos:inScheme sector-law:purposes-classes ;
    skos:prefLabel "Unauthorised Migration Detection"@en .

sector-law:UnauthorisedMigrationManagement a rdfs:Class,
        skos:Concept,
        dpv:Purpose ;
    dct:created "2024-12-01"^^xsd:date ;
    rdfs:isDefinedBy sector-law: ;
    sw:term_status "accepted"@en ;
    skos:broader sector-law:ImmigrationSecurityManagement ;
    skos:definition "Puposes associated with detection, prevention, and management of unauthorised migration within the legal system"@en ;
    skos:inScheme sector-law:purposes-classes ;
    skos:prefLabel "Unauthorised Migration Management"@en .

sector-law:UnauthorisedMigrationPrediction a rdfs:Class,
        skos:Concept,
        dpv:Purpose ;
    dct:created "2024-12-01"^^xsd:date ;
    rdfs:isDefinedBy sector-law: ;
    sw:term_status "accepted"@en ;
    skos:broader sector-law:UnauthorisedMigrationManagement ;
    skos:definition "Puposes associated with predicting unauthorised migration within the legal system"@en ;
    skos:inScheme sector-law:purposes-classes ;
    skos:prefLabel "Unauthorised Migration Prediction"@en .

<https://w3id.org/dpv/sector/law> a owl:Ontology,
        profile:Profile ;
    dct:bibliographicCitation "Harshvardhan J. Pandit, Beatriz Esteves, Georg P. Krog, Paul Ryan, Delaram Golpayegani, Julian Flake (2025) Data Privacy Vocabulary (DPV) – Version 2.0. In: Demartini, G., et al. The Semantic Web – ISWC 2024. ISWC 2024. Lecture Notes in Computer Science, vol 15233. Springer, Cham. https://doi.org/10.1007/978-3-031-77847-6_10" ;
    dct:conformsTo "http://www.w3.org/2000/01/rdf-schema",
        "http://www.w3.org/2004/02/skos/core" ;
    dct:created "2024-12-01"@en ;
    dct:creator [ a dct:Agent,
                foaf:Person ;
            scoro:hasORCID "0000-0002-5068-3714" ;
            org:memberOf [ a foaf:Organization ;
                    foaf:name "ADAPT Centre, Dublin City University" ] ;
            foaf:homepage "https://harshp.com/" ;
            foaf:name "Harshvardhan J. Pandit" ] ;
    dct:description "Extension to the Data Privacy Vocabulary (DPV) providing concepts for the law enforcement and justice sector"@en ;
    dct:identifier "https://w3id.org/dpv/sector/law" ;
    dct:issued "2024-12-01"@en ;
    dct:license <https://www.w3.org/copyright/document-license-2023/> ;
    dct:modified "2025-03-16"@en ;
    dct:publisher <https://www.w3.org/> ;
    dct:source <https://www.w3.org/groups/cg/dpvcg/> ;
    dct:title "Law Enforcement & Justice Sector Concepts"@en ;
    bibo:doi "10.5281/zenodo.12505841" ;
    bibo:status "http://purl.org/ontology/bibo/status/draft" ;
    vann:preferredNamespacePrefix "sector-law" ;
    vann:preferredNamespaceUri "https://w3id.org/dpv/sector/law#" ;
    rdfs:Label "SECTOR-LAW"@en ;
    owl:versionIRI <https://w3id.org/dpv/2.1/sector/law> ;
    owl:versionInfo "2.1" ;
    profile:hasResource <https://w3id.org/dpv/examples>,
        <https://w3id.org/dpv/guides>,
        <https://w3id.org/dpv/primer>,
        sector-law:serialisation-html,
        sector-law:serialisation-jsonld,
        sector-law:serialisation-n3,
        sector-law:serialisation-rdf,
        sector-law:serialisation-ttl ;
    profile:isProfileOf rdfs:,
        skos:,
        <https://w3id.org/dpv> ;
    foaf:logo <https://w3id.org/dpv/media/logo.png> ;
    schema:version "2.1" .

sector-law:serialisation-html a profile:ResourceDescriptor ;
    dct:conformsTo <https://www.w3.org/TR/html/> ;
    dct:format <https://www.iana.org/assignments/media-types/text/html> ;
    dct:title "Law Enforcement & Justice Sector Concepts - HTML serialiation" ;
    profile:hasArtifact <https://w3id.org/dpv/sector/law/sector-law.html> ;
    profile:hasRole role:specification .

sector-law:serialisation-jsonld a profile:ResourceDescriptor ;
    dct:conformsTo <https://www.w3.org/TR/json-ld11/> ;
    dct:format <https://www.iana.org/assignments/media-types/application/ld+json> ;
    dct:title "Law Enforcement & Justice Sector Concepts - JSON-LD serialiation" ;
    profile:hasArtifact <https://w3id.org/dpv/sector/law/sector-law.jsonld> ;
    profile:hasRole role:vocabulary .

sector-law:serialisation-n3 a profile:ResourceDescriptor ;
    dct:conformsTo <https://www.w3.org/TeamSubmission/n3/> ;
    dct:format <https://www.iana.org/assignments/media-types/text/n3> ;
    dct:title "Law Enforcement & Justice Sector Concepts - N3 serialiation" ;
    profile:hasArtifact <https://w3id.org/dpv/sector/law/sector-law.n3> ;
    profile:hasRole role:vocabulary .

sector-law:serialisation-rdf a profile:ResourceDescriptor ;
    dct:conformsTo rdf: ;
    dct:format <https://www.iana.org/assignments/media-types/application/rdf+xml> ;
    dct:title "Law Enforcement & Justice Sector Concepts - RDF/XML serialiation" ;
    profile:hasArtifact <https://w3id.org/dpv/sector/law/sector-law.rdf> ;
    profile:hasRole role:vocabulary .

sector-law:serialisation-ttl a profile:ResourceDescriptor ;
    dct:conformsTo <https://www.w3.org/TR/turtle/> ;
    dct:format <https://www.iana.org/assignments/media-types/text/turtle> ;
    dct:title "Law Enforcement & Justice Sector Concepts - Turtle serialiation" ;
    profile:hasArtifact <https://w3id.org/dpv/sector/law/sector-law.ttl> ;
    profile:hasRole role:vocabulary .

<https://w3id.org/dpv/examples> a profile:ResourceDescriptor ;
    dct:conformsTo <https://www.w3.org/TR/html/> ;
    dct:format <https://www.iana.org/assignments/media-types/text/html> ;
    dct:title "Examples for Data Privacy Vocabulary" ;
    profile:hasArtifact <https://w3id.org/dpv/examples> ;
    profile:hasRole role:guidance .

<https://w3id.org/dpv/guides> a profile:ResourceDescriptor ;
    dct:conformsTo <https://www.w3.org/TR/html/> ;
    dct:format <https://www.iana.org/assignments/media-types/text/html> ;
    dct:title "Guides for Data Privacy Vocabulary" ;
    profile:hasArtifact <https://w3id.org/dpv/guides> ;
    profile:hasRole role:guidance .

<https://w3id.org/dpv/primer> a profile:ResourceDescriptor ;
    dct:conformsTo <https://www.w3.org/TR/html/> ;
    dct:format <https://www.iana.org/assignments/media-types/text/html> ;
    dct:title "Primer for Data Privacy Vocabulary" ;
    profile:hasArtifact <https://w3id.org/dpv/primer> ;
    profile:hasRole role:guidance .

sector-law:purposes-classes a skos:ConceptScheme .

