<?xml version="1.0" encoding="utf-8"?>
<rdf:RDF
   xmlns:bibo="http://purl.org/ontology/bibo/"
   xmlns:dcam="http://purl.org/dc/dcam/"
   xmlns:dct="http://purl.org/dc/terms/"
   xmlns:foaf="http://xmlns.com/foaf/0.1/"
   xmlns:org="http://www.w3.org/ns/org#"
   xmlns:owl="http://www.w3.org/2002/07/owl#"
   xmlns:profile="http://www.w3.org/ns/dx/prof/"
   xmlns:rdf="http://www.w3.org/1999/02/22-rdf-syntax-ns#"
   xmlns:rdfs="http://www.w3.org/2000/01/rdf-schema#"
   xmlns:schema="https://schema.org/"
   xmlns:scoro="http://purl.org/spar/scoro/"
   xmlns:skos="http://www.w3.org/2004/02/skos/core#"
   xmlns:sw="http://www.w3.org/2003/06/sw-vocab-status/ns#"
   xmlns:vann="http://purl.org/vocab/vann/"
>
  <rdf:Description rdf:about="https://w3id.org/dpv/legal/de/gdng/owl#FederalStateCentresForCancerRegistryData">
    <rdf:type rdf:resource="http://www.w3.org/2000/01/rdf-schema#Class"/>
    <rdf:type rdf:resource="http://www.w3.org/2002/07/owl#Class"/>
    <dct:created rdf:datatype="http://www.w3.org/2001/XMLSchema#date">2025-10-13</dct:created>
    <dct:source xml:lang="en">[[GDNG]] § 3(2) point 10</dct:source>
    <skos:prefLabel xml:lang="de">klinische Krebsregister der Länder</skos:prefLabel>
    <skos:prefLabel xml:lang="en">Federal State Centres for Cancer Registry Data</skos:prefLabel>
    <rdfs:subClassOf rdf:resource="https://w3id.org/dpv/legal/de/gdng/owl#HealthDataHolder"/>
    <dct:contributor rdf:nodeID="person-julian-flake"/>
    <skos:definition xml:lang="en">The federal state centres for cancer registry data pursuant to § 65c des Fünften Buches Sozialgesetzbuch</skos:definition>
    <skos:definition xml:lang="de">Die klinischen Krebsregister der Länder nach § 65c des Fünften Buches Sozialgesetzbuch</skos:definition>
    <rdfs:isDefinedBy rdf:resource="https://w3id.org/dpv/legal/de/gdng/owl#"/>
    <sw:term_status xml:lang="en">accepted</sw:term_status>
  </rdf:Description>
  <rdf:Description rdf:about="https://w3id.org/dpv/legal/de/gdng/owl#AuthorizedPerson">
    <rdf:type rdf:resource="http://www.w3.org/2000/01/rdf-schema#Class"/>
    <rdf:type rdf:resource="http://www.w3.org/2002/07/owl#Class"/>
    <sw:term_status xml:lang="en">accepted</sw:term_status>
    <skos:prefLabel xml:lang="de">Befugte Person</skos:prefLabel>
    <skos:prefLabel xml:lang="en">Authorized Person</skos:prefLabel>
    <skos:definition xml:lang="en">A natural person that, according to a rights and rolls concept, proccesses healtcare data at a healthcare facility pursuant to the legal basis of § 6(1) GDNG</skos:definition>
    <skos:definition xml:lang="de">Eine natürliche Person die nach einem Rechte- und Rollenkonzept die Weiterverarbeitung von Gesundheitsdaten nach der Rechtsgrundlage § 6(1) GDNG an einer Gesundheitseinrichtung durchführt</skos:definition>
    <rdfs:isDefinedBy rdf:resource="https://w3id.org/dpv/legal/de/gdng/owl#"/>
    <dct:created rdf:datatype="http://www.w3.org/2001/XMLSchema#date">2025-10-13</dct:created>
    <dct:source xml:lang="en">[[GDNG]] § 6(1)</dct:source>
    <dct:contributor rdf:nodeID="person-julian-flake"/>
  </rdf:Description>
  <rdf:Description rdf:about="https://w3id.org/dpv/legal/de/gdng/owl#HealthDataLab">
    <skos:prefLabel xml:lang="de">Forschungsdatenzentrum Gesundheit</skos:prefLabel>
    <skos:prefLabel xml:lang="en">Health Data Lab</skos:prefLabel>
    <rdfs:isDefinedBy rdf:resource="https://w3id.org/dpv/legal/de/gdng/owl#"/>
    <dct:created rdf:datatype="http://www.w3.org/2001/XMLSchema#date">2025-10-13</dct:created>
    <dct:contributor rdf:nodeID="person-julian-flake"/>
    <dct:contributor rdf:nodeID="person-christian-draeger"/>
    <dct:source xml:lang="en">[[GDNG]] § 2</dct:source>
    <rdf:type rdf:resource="http://www.w3.org/2000/01/rdf-schema#Class"/>
    <rdf:type rdf:resource="https://w3id.org/dpv/legal/de/gdng/owl#RegulatedHealthDataHolder"/>
    <rdf:type rdf:resource="http://www.w3.org/2002/07/owl#Class"/>
    <sw:term_status xml:lang="en">accepted</sw:term_status>
    <skos:definition xml:lang="en">Health Data Lab pursuant to § 303d of Fünftes Buch Sozialgesetzbuch</skos:definition>
    <skos:definition xml:lang="de">Forschungsdatenzentrum Gesundheit nach § 303d des Fünften Buches Sozialgesetzbuch</skos:definition>
    <rdfs:subClassOf rdf:resource="https://w3id.org/dpv/legal/de/gdng/owl#RegulatedHealthDataHolder"/>
  </rdf:Description>
  <rdf:Description rdf:about="https://w3id.org/dpv/legal/de/gdng/owl#">
    <owl:versionIRI rdf:resource="https://w3id.org/dpv/2.3/legal/de/gdng/owl#"/>
    <profile:hasResource rdf:resource="https://w3id.org/dpv/legal/de/gdng/owl#serialisation-ttl"/>
    <profile:hasResource rdf:resource="https://w3id.org/dpv/guides"/>
    <profile:hasResource rdf:resource="https://w3id.org/dpv/legal/de/gdng/owl#serialisation-rdf"/>
    <profile:hasResource rdf:resource="https://w3id.org/dpv/primer"/>
    <profile:hasResource rdf:resource="https://w3id.org/dpv/legal/de/gdng/owl#serialisation-html"/>
    <profile:hasResource rdf:resource="https://w3id.org/dpv/examples"/>
    <profile:hasResource rdf:resource="https://w3id.org/dpv/legal/de/gdng/owl#serialisation-n3"/>
    <profile:hasResource rdf:resource="https://w3id.org/dpv/legal/de/gdng/owl#serialisation-jsonld"/>
    <dct:title xml:lang="en">Legal Concepts for German Gesundheitsdatennutzungsgesetz (DE)</dct:title>
    <dct:issued xml:lang="en">2026-01-21</dct:issued>
    <dct:conformsTo>http://www.w3.org/2004/02/skos/core</dct:conformsTo>
    <dct:conformsTo rdf:resource="http://www.w3.org/2002/07/owl"/>
    <dct:conformsTo>http://www.w3.org/2000/01/rdf-schema</dct:conformsTo>
    <dct:description xml:lang="en">Extension to the Data Privacy Vocabulary (DPV) providing concepts for representing legal information for a German regulation</dct:description>
    <dct:creator rdf:nodeID="person-julian-flake"/>
    <dct:creator rdf:nodeID="person-christian-draeger"/>
    <dct:source rdf:resource="https://www.w3.org/groups/cg/dpvcg/"/>
    <profile:isProfileOf rdf:resource="https://w3id.org/dpv/owl"/>
    <profile:isProfileOf rdf:resource="http://www.w3.org/2002/07/owl"/>
    <profile:isProfileOf rdf:resource="https://w3id.org/dpv/legal/de/gdng/owl#"/>
    <rdf:type rdf:resource="http://www.w3.org/2002/07/owl#Ontology"/>
    <rdf:type rdf:resource="http://www.w3.org/ns/dx/prof/Profile"/>
    <dct:created xml:lang="en">2026-01-21</dct:created>
    <dct:hasVersion rdf:resource="https://w3id.org/dpv/legal/de/gdng/owl#"/>
    <schema:version>2.3</schema:version>
    <foaf:logo rdf:resource="https://w3id.org/dpv/media/logo.png"/>
    <vann:preferredNamespacePrefix>de-gdng</vann:preferredNamespacePrefix>
    <bibo:status>http://purl.org/ontology/bibo/status/draft</bibo:status>
    <dct:identifier>https://w3id.org/dpv/legal/de/gdng</dct:identifier>
    <vann:preferredNamespaceUri>https://w3id.org/dpv/legal/de/gdng#</vann:preferredNamespaceUri>
    <dct:contributor rdf:nodeID="person-julian-flake"/>
    <dct:contributor rdf:nodeID="person-christian-draeger"/>
    <dct:publisher rdf:resource="https://www.w3.org/"/>
    <dct:license rdf:resource="https://www.w3.org/copyright/document-license-2023/"/>
    <dct:modified xml:lang="en">2026-02-25</dct:modified>
    <bibo:doi>10.5281/zenodo.12505841</bibo:doi>
    <dct:bibliographicCitation>Harshvardhan J. Pandit, Beatriz Esteves, Georg P. Krog, Paul Ryan, Delaram Golpayegani, Julian Flake (2025) Data Privacy Vocabulary (DPV) – Version 2.0. In: Demartini, G., et al. The Semantic Web – ISWC 2024. ISWC 2024. Lecture Notes in Computer Science, vol 15233. Springer, Cham. https://doi.org/10.1007/978-3-031-77847-6_10</dct:bibliographicCitation>
    <owl:versionInfo>2.3</owl:versionInfo>
    <rdfs:Label xml:lang="en">DE-GDNG</rdfs:Label>
  </rdf:Description>
  <rdf:Description rdf:about="https://w3id.org/dpv/legal/de/gdng/owl#HealthDataHolder">
    <dct:contributor rdf:nodeID="person-julian-flake"/>
    <skos:definition xml:lang="en">Natural or legal person that is authorised or obligated to process health data for research purposes</skos:definition>
    <skos:definition xml:lang="de">Natürliche oder juristische Personen, die berechtigt oder verpflichtet sind, Gesundheitsdaten für Forschungszwecke zu verarbeiten</skos:definition>
    <dct:source xml:lang="en">[[GDNG]] § 2(3)</dct:source>
    <sw:term_status xml:lang="en">accepted</sw:term_status>
    <rdf:type rdf:resource="http://www.w3.org/2000/01/rdf-schema#Class"/>
    <rdf:type rdf:resource="http://www.w3.org/2002/07/owl#Class"/>
    <dct:created rdf:datatype="http://www.w3.org/2001/XMLSchema#date">2025-10-13</dct:created>
    <skos:prefLabel xml:lang="de">Datenhaltende Stelle</skos:prefLabel>
    <skos:prefLabel xml:lang="en">Health Data Holder</skos:prefLabel>
    <rdfs:isDefinedBy rdf:resource="https://w3id.org/dpv/legal/de/gdng/owl#"/>
  </rdf:Description>
  <rdf:Description rdf:about="https://w3id.org/dpv/legal/de/gdng/owl#hasDataHolder">
    <rdf:type rdf:resource="http://www.w3.org/1999/02/22-rdf-syntax-ns#Property"/>
    <rdf:type rdf:resource="http://www.w3.org/2002/07/owl#ObjectProperty"/>
    <rdfs:isDefinedBy rdf:resource="https://w3id.org/dpv/legal/de/gdng/owl#"/>
    <schema:rangeIncludes rdf:resource="https://w3id.org/dpv/legal/de/gdng/owl#DataHolder"/>
    <dct:created rdf:datatype="http://www.w3.org/2001/XMLSchema#date">2026-01-22</dct:created>
    <dct:contributor rdf:nodeID="person-julian-flake"/>
    <skos:related rdf:resource="https://w3id.org/dpv/legal/de/gdng/owl#DataHolder"/>
    <sw:term_status xml:lang="en">accepted</sw:term_status>
    <skos:definition xml:lang="en">something is related to a data holder</skos:definition>
    <skos:prefLabel xml:lang="en">has Data Holder</skos:prefLabel>
    <dcam:rangeIncludes rdf:resource="https://w3id.org/dpv/legal/de/gdng/owl#DataHolder"/>
    <rdfs:subPropertyOf rdf:resource="https://w3id.org/dpv/owl#hasEntity"/>
  </rdf:Description>
  <rdf:Description rdf:about="https://w3id.org/dpv/examples">
    <profile:hasArtifact rdf:resource="https://w3id.org/dpv/examples"/>
    <profile:hasRole rdf:resource="http://www.w3.org/ns/dx/prof/role/guidance"/>
    <dct:format rdf:resource="https://www.iana.org/assignments/media-types/text/html"/>
    <dct:title>Examples</dct:title>
    <dct:conformsTo rdf:resource="https://www.w3.org/TR/html/"/>
    <rdf:type rdf:resource="http://www.w3.org/ns/dx/prof/ResourceDescriptor"/>
  </rdf:Description>
  <rdf:Description rdf:about="https://w3id.org/dpv/legal/de/gdng/owl#ResponsibleDataHoldingAndMediatingBody">
    <rdfs:subClassOf rdf:resource="https://w3id.org/dpv/legal/de/gdng/owl#HealthDataHolder"/>
    <dct:contributor rdf:nodeID="person-christian-draeger"/>
    <dct:contributor rdf:nodeID="person-julian-flake"/>
    <rdfs:isDefinedBy rdf:resource="https://w3id.org/dpv/legal/de/gdng/owl#"/>
    <dct:created rdf:datatype="http://www.w3.org/2001/XMLSchema#date">2025-10-13</dct:created>
    <skos:prefLabel xml:lang="en">Responsible Data-holding and Mediating Body</skos:prefLabel>
    <skos:prefLabel xml:lang="de">Zuständige datenhaltende und mittelnde Stelle</skos:prefLabel>
    <dct:source xml:lang="en">[[GDNG]] § 3(2) point 4</dct:source>
    <skos:definition xml:lang="de">Diejenige datenhaltende und -mittelnde Stelle, die für ein konkretes Forschungsvorhaben zuständig ist</skos:definition>
    <skos:definition xml:lang="en">Data holding and mediating body responsible for a specific research project</skos:definition>
    <rdf:type rdf:resource="http://www.w3.org/2000/01/rdf-schema#Class"/>
    <rdf:type rdf:resource="http://www.w3.org/2002/07/owl#Class"/>
    <sw:term_status xml:lang="en">accepted</sw:term_status>
  </rdf:Description>
  <rdf:Description rdf:about="https://w3id.org/dpv/legal/de/gdng/owl#HealthDataUser">
    <sw:term_status xml:lang="en">accepted</sw:term_status>
    <skos:prefLabel xml:lang="de">Datennutzende</skos:prefLabel>
    <skos:prefLabel xml:lang="en">Health Data User</skos:prefLabel>
    <rdf:type rdf:resource="http://www.w3.org/2000/01/rdf-schema#Class"/>
    <rdf:type rdf:resource="http://www.w3.org/2002/07/owl#Class"/>
    <dct:created rdf:datatype="http://www.w3.org/2001/XMLSchema#date">2025-10-13</dct:created>
    <skos:definition xml:lang="de">Natürliche und juristische Personen, die Zugang zu Gesundheitsdaten zu Forschungszwecken und weiteren Zwecken begehren oder erhalten haben</skos:definition>
    <skos:definition xml:lang="en">Natural or legal person that is requesting or entitled to process health data for research purposes</skos:definition>
    <rdfs:isDefinedBy rdf:resource="https://w3id.org/dpv/legal/de/gdng/owl#"/>
    <dct:contributor rdf:nodeID="person-julian-flake"/>
    <dct:source xml:lang="en">[[GDNG]] § 2</dct:source>
  </rdf:Description>
  <rdf:Description rdf:about="https://w3id.org/dpv/legal/de/gdng/owl#RegulatedHealthDataHolder">
    <dct:source xml:lang="en">[[GDNG]] § 2(3)</dct:source>
    <rdfs:subClassOf rdf:resource="https://w3id.org/dpv/legal/de/gdng/owl#HealthDataHolder"/>
    <rdf:type rdf:resource="http://www.w3.org/2000/01/rdf-schema#Class"/>
    <rdf:type rdf:resource="http://www.w3.org/2002/07/owl#Class"/>
    <rdfs:isDefinedBy rdf:resource="https://w3id.org/dpv/legal/de/gdng/owl#"/>
    <skos:prefLabel xml:lang="de">Gesetzlich geregelte datenhaltende Stelle</skos:prefLabel>
    <skos:prefLabel xml:lang="en">Regulated Health Data Holder</skos:prefLabel>
    <dct:created rdf:datatype="http://www.w3.org/2001/XMLSchema#date">2025-10-13</dct:created>
    <dct:contributor rdf:nodeID="person-julian-flake"/>
    <skos:definition xml:lang="en">Data holders regulated by law. Examples are the German "Health Data Lab", the "German Centre for Cancer Registry Data" and the "Model Project Genome Sequencing"</skos:definition>
    <skos:definition xml:lang="de">Solche datenhaltenden Stellen, die gesetzlich geregelt sind, wie das Forschungsdatenzentrum Gesundheit, das Zentrum für Krebregisterdaten beim RKI und die Plattform nach §64e Abs.9 des fünften Buches Sozialgesetzbuch</skos:definition>
    <sw:term_status xml:lang="en">accepted</sw:term_status>
  </rdf:Description>
  <rdf:Description rdf:nodeID="org-university-of-koblenz">
    <foaf:name>University of Koblenz</foaf:name>
    <rdf:type rdf:resource="http://xmlns.com/foaf/0.1/Organization"/>
  </rdf:Description>
  <rdf:Description rdf:about="https://w3id.org/dpv/legal/de/gdng/owl#Controller">
    <dct:contributor rdf:nodeID="person-julian-flake"/>
    <dct:contributor rdf:nodeID="person-christian-draeger"/>
    <skos:prefLabel xml:lang="de">Datenschutzrechtlich verantwortliche Stelle</skos:prefLabel>
    <skos:prefLabel xml:lang="en">Controller</skos:prefLabel>
    <rdfs:isDefinedBy rdf:resource="https://w3id.org/dpv/legal/de/gdng/owl#"/>
    <dct:created rdf:datatype="http://www.w3.org/2001/XMLSchema#date">2026-02-08</dct:created>
    <rdf:type rdf:resource="http://www.w3.org/2000/01/rdf-schema#Class"/>
    <rdf:type rdf:resource="http://www.w3.org/2002/07/owl#Class"/>
    <sw:term_status xml:lang="en">accepted</sw:term_status>
    <dct:source xml:lang="en">[[GDNG]] § 6(3)</dct:source>
  </rdf:Description>
  <rdf:Description rdf:about="https://w3id.org/dpv/legal/de/gdng/owl#serialisation-ttl">
    <profile:hasArtifact rdf:resource="https://w3id.org/dpv/legal/de/gdng/de-gdng-owl.ttl"/>
    <dct:format rdf:resource="https://www.iana.org/assignments/media-types/text/turtle"/>
    <profile:hasRole rdf:resource="http://www.w3.org/ns/dx/prof/role/vocabulary"/>
    <dct:title>Legal Concepts for German Gesundheitsdatennutzungsgesetz (DE) - Turtle serialisation</dct:title>
    <rdf:type rdf:resource="http://www.w3.org/ns/dx/prof/ResourceDescriptor"/>
    <dct:conformsTo rdf:resource="https://www.w3.org/TR/turtle/"/>
  </rdf:Description>
  <rdf:Description rdf:about="https://w3id.org/dpv/legal/de/gdng/owl#ThirdParty">
    <rdfs:isDefinedBy rdf:resource="https://w3id.org/dpv/legal/de/gdng/owl#"/>
    <skos:prefLabel xml:lang="de">Dritte</skos:prefLabel>
    <skos:prefLabel xml:lang="en">Third Party</skos:prefLabel>
    <dct:contributor rdf:nodeID="person-julian-flake"/>
    <dct:contributor rdf:nodeID="person-christian-draeger"/>
    <dct:source xml:lang="en">[[GDNG]] § 6(3)</dct:source>
    <sw:term_status xml:lang="en">accepted</sw:term_status>
    <rdf:type rdf:resource="http://www.w3.org/2000/01/rdf-schema#Class"/>
    <rdf:type rdf:resource="http://www.w3.org/2002/07/owl#Class"/>
    <dct:created rdf:datatype="http://www.w3.org/2001/XMLSchema#date">2026-02-10</dct:created>
  </rdf:Description>
  <rdf:Description rdf:about="https://w3id.org/dpv/legal/de/gdng/owl#ModelProjectGenomeSequencingPlatform">
    <rdf:type rdf:resource="http://www.w3.org/2000/01/rdf-schema#Class"/>
    <rdf:type rdf:resource="https://w3id.org/dpv/legal/de/gdng/owl#RegulatedHealthDataHolder"/>
    <rdf:type rdf:resource="http://www.w3.org/2002/07/owl#Class"/>
    <skos:prefLabel xml:lang="de">Plattform des Modellvorhabens Genomsequenzierung</skos:prefLabel>
    <skos:prefLabel xml:lang="en">Model Project Genome Sequencing Platform</skos:prefLabel>
    <rdfs:isDefinedBy rdf:resource="https://w3id.org/dpv/legal/de/gdng/owl#"/>
    <skos:definition xml:lang="en">Model Project Platform pursuant to § 64e of Fünften Buches Sozialgesetzbuch</skos:definition>
    <skos:definition xml:lang="de">Plattform nach § 64e Modellvorhaben zur umfassenden Diagnostik und Therapiefindung mittels Genomsequenzierung bei seltenen und bei onkologischen Erkrankungen, Verordnungsermächtigung des Fünften Buches Sozialgesetzbuch</skos:definition>
    <dct:contributor rdf:nodeID="person-christian-draeger"/>
    <dct:contributor rdf:nodeID="person-julian-flake"/>
    <dct:source xml:lang="en">[[GDNG]] § 2</dct:source>
    <sw:term_status xml:lang="en">accepted</sw:term_status>
    <dct:created rdf:datatype="http://www.w3.org/2001/XMLSchema#date">2025-10-13</dct:created>
    <rdfs:subClassOf rdf:resource="https://w3id.org/dpv/legal/de/gdng/owl#RegulatedHealthDataHolder"/>
  </rdf:Description>
  <rdf:Description rdf:about="https://w3id.org/dpv/legal/de/gdng/owl#DataInfrastructure">
    <rdfs:isDefinedBy rdf:resource="https://w3id.org/dpv/legal/de/gdng/owl#"/>
    <dct:created rdf:datatype="http://www.w3.org/2001/XMLSchema#date">2025-10-13</dct:created>
    <skos:definition xml:lang="en">Networks of health data holders forming data infrastructures</skos:definition>
    <skos:definition xml:lang="de">Zusammenschlüsse von datenhaltenden Stellen zu Dateninfrastrukturen</skos:definition>
    <dct:contributor rdf:nodeID="person-christian-draeger"/>
    <dct:contributor rdf:nodeID="person-julian-flake"/>
    <sw:term_status xml:lang="en">accepted</sw:term_status>
    <rdf:type rdf:resource="http://www.w3.org/2000/01/rdf-schema#Class"/>
    <rdf:type rdf:resource="http://www.w3.org/2002/07/owl#Class"/>
    <rdfs:subClassOf rdf:resource="https://w3id.org/dpv/legal/de/gdng/owl#HealthDataHolder"/>
    <skos:prefLabel xml:lang="de">Dateninfrastruktur</skos:prefLabel>
    <skos:prefLabel xml:lang="en">Data Infrastructure</skos:prefLabel>
    <dct:source xml:lang="en">[[GDNG]] § 2</dct:source>
  </rdf:Description>
  <rdf:Description rdf:about="https://w3id.org/dpv/legal/de/gdng/owl#DataSubject">
    <dct:contributor rdf:nodeID="person-christian-draeger"/>
    <dct:contributor rdf:nodeID="person-julian-flake"/>
    <sw:term_status xml:lang="en">accepted</sw:term_status>
    <skos:prefLabel xml:lang="en">Data Subject</skos:prefLabel>
    <skos:prefLabel xml:lang="de">Betroffene Person</skos:prefLabel>
    <dct:source xml:lang="en">[[GDNG]] § 6(3)</dct:source>
    <rdf:type rdf:resource="http://www.w3.org/2000/01/rdf-schema#Class"/>
    <rdf:type rdf:resource="http://www.w3.org/2002/07/owl#Class"/>
    <rdfs:isDefinedBy rdf:resource="https://w3id.org/dpv/legal/de/gdng/owl#"/>
    <dct:created rdf:datatype="http://www.w3.org/2001/XMLSchema#date">2026-02-08</dct:created>
  </rdf:Description>
  <rdf:Description rdf:about="https://w3id.org/dpv/legal/de/gdng/owl#serialisation-html">
    <profile:hasArtifact rdf:resource="https://w3id.org/dpv/legal/de/gdng/de-gdng-owl.html"/>
    <dct:title>Legal Concepts for German Gesundheitsdatennutzungsgesetz (DE) - HTML serialisation</dct:title>
    <dct:format rdf:resource="https://www.iana.org/assignments/media-types/text/html"/>
    <profile:hasRole rdf:resource="http://www.w3.org/ns/dx/prof/role/specification"/>
    <dct:conformsTo rdf:resource="https://www.w3.org/TR/html/"/>
    <rdf:type rdf:resource="http://www.w3.org/ns/dx/prof/ResourceDescriptor"/>
  </rdf:Description>
  <rdf:Description rdf:about="https://w3id.org/dpv/legal/de/gdng/owl#PublicJointHealthResearchNetwork">
    <dct:created rdf:datatype="http://www.w3.org/2001/XMLSchema#date">2025-10-13</dct:created>
    <skos:definition xml:lang="en">Publicly funded networks of data processing healthcare facilitys, including joint research projects and research practice networks, which jointly use and process health data pursuant to § 6(1) GDNG</skos:definition>
    <skos:definition xml:lang="de">Öffentlich geförderte Zusammenschlüsse von datenverarbeitenden Gesundheitseinrichtungen einschließlich Verbundforschungsvorhaben und Forschungspraxennetzwerken, die nach § 6(1) GDNG Gesundheitsdaten gemeinsam nutzen und verarbeiten</skos:definition>
    <skos:prefLabel xml:lang="en">Publicly Funded Networks of Data Processing Healthcare Facilitys</skos:prefLabel>
    <skos:prefLabel xml:lang="de">Öffentlich geförderte Zusammenschlüsse von datenverarbeitenden Gesundheitseinrichtungen</skos:prefLabel>
    <dct:contributor rdf:nodeID="person-julian-flake"/>
    <dct:contributor rdf:nodeID="person-christian-draeger"/>
    <dct:source xml:lang="en">[[GDNG]] § 6(3)</dct:source>
    <sw:term_status xml:lang="en">accepted</sw:term_status>
    <rdf:type rdf:resource="http://www.w3.org/2000/01/rdf-schema#Class"/>
    <rdf:type rdf:resource="http://www.w3.org/2002/07/owl#Class"/>
    <rdfs:isDefinedBy rdf:resource="https://w3id.org/dpv/legal/de/gdng/owl#"/>
  </rdf:Description>
  <rdf:Description rdf:about="https://w3id.org/dpv/legal/de/gdng/owl#DataAccessAndCoordinationOffice">
    <skos:definition xml:lang="de">Datenzugangs- und Koordinierungsstelle für Gesundheitsdaten (DACO), angesiedelt beim Bundesinstitut für Arzneimittel und Medizinprodukte (BfArM)</skos:definition>
    <skos:definition xml:lang="en">Data Access and Coordination Office for Health Data (DACO), based at the Federal Institute for Drugs and Medical Devices (BfArM)</skos:definition>
    <sw:term_status xml:lang="en">accepted</sw:term_status>
    <rdf:type rdf:resource="http://www.w3.org/2000/01/rdf-schema#Class"/>
    <rdf:type rdf:resource="https://w3id.org/dpv/owl#Authority"/>
    <rdf:type rdf:resource="http://www.w3.org/2002/07/owl#Class"/>
    <dct:source xml:lang="en">[[GDNG]] § 3(1)</dct:source>
    <rdfs:isDefinedBy rdf:resource="https://w3id.org/dpv/legal/de/gdng/owl#"/>
    <skos:prefLabel xml:lang="en">Data Access and Coordination Office (DACO)</skos:prefLabel>
    <skos:prefLabel xml:lang="de">Datenzugangs- und Koordinierungsstelle für Gesundheitsdaten (DACO)</skos:prefLabel>
    <dct:created rdf:datatype="http://www.w3.org/2001/XMLSchema#date">2025-10-13</dct:created>
    <dct:contributor rdf:nodeID="person-julian-flake"/>
    <rdfs:subClassOf rdf:resource="https://w3id.org/dpv/owl#Authority"/>
  </rdf:Description>
  <rdf:Description rdf:about="https://w3id.org/dpv/legal/de/gdng/owl#GermanCentreForCancerRegistryData">
    <rdf:type rdf:resource="http://www.w3.org/2000/01/rdf-schema#Class"/>
    <rdf:type rdf:resource="https://w3id.org/dpv/legal/de/gdng/owl#RegulatedHealthDataHolder"/>
    <rdf:type rdf:resource="http://www.w3.org/2002/07/owl#Class"/>
    <skos:definition xml:lang="de">Zentrum für Krebsregisterdaten nach § 1 Bundeskrebsregisterdaten­gesetz</skos:definition>
    <skos:definition xml:lang="en">German Centre for Cancer Registry Data pursuant § 1 Bundeskrebsregisterdatengesetz</skos:definition>
    <skos:prefLabel xml:lang="de">Zentrum für Krebsregisterdaten beim Robert-Koch-Institut</skos:prefLabel>
    <skos:prefLabel xml:lang="en">German Centre for Cancer Registry Data</skos:prefLabel>
    <rdfs:isDefinedBy rdf:resource="https://w3id.org/dpv/legal/de/gdng/owl#"/>
    <dct:created rdf:datatype="http://www.w3.org/2001/XMLSchema#date">2025-10-13</dct:created>
    <dct:contributor rdf:nodeID="person-christian-draeger"/>
    <dct:contributor rdf:nodeID="person-julian-flake"/>
    <dct:source xml:lang="en">[[GDNG]] § 2</dct:source>
    <sw:term_status xml:lang="en">accepted</sw:term_status>
    <rdfs:subClassOf rdf:resource="https://w3id.org/dpv/legal/de/gdng/owl#RegulatedHealthDataHolder"/>
  </rdf:Description>
  <rdf:Description rdf:about="https://w3id.org/dpv/legal/de/gdng/owl#DataPlatform">
    <dct:contributor rdf:nodeID="person-christian-draeger"/>
    <dct:contributor rdf:nodeID="person-julian-flake"/>
    <dct:source xml:lang="en">[[GDNG]] § 2</dct:source>
    <sw:term_status xml:lang="en">accepted</sw:term_status>
    <rdf:type rdf:resource="http://www.w3.org/2000/01/rdf-schema#Class"/>
    <rdf:type rdf:resource="http://www.w3.org/2002/07/owl#Class"/>
    <dct:created rdf:datatype="http://www.w3.org/2001/XMLSchema#date">2025-10-13</dct:created>
    <skos:definition xml:lang="en">Networks of health data holders forming data platforms</skos:definition>
    <skos:definition xml:lang="de">Zusammenschlüsse von datenhaltenden Stellen zu Datenplattformen</skos:definition>
    <skos:prefLabel xml:lang="en">Data Platform</skos:prefLabel>
    <skos:prefLabel xml:lang="de">Datenplattform</skos:prefLabel>
    <rdfs:subClassOf rdf:resource="https://w3id.org/dpv/legal/de/gdng/owl#HealthDataHolder"/>
    <rdfs:isDefinedBy rdf:resource="https://w3id.org/dpv/legal/de/gdng/owl#"/>
  </rdf:Description>
  <rdf:Description rdf:about="https://w3id.org/dpv/legal/de/gdng/owl#serialisation-jsonld">
    <dct:title>Legal Concepts for German Gesundheitsdatennutzungsgesetz (DE) - JSON-LD serialisation</dct:title>
    <rdf:type rdf:resource="http://www.w3.org/ns/dx/prof/ResourceDescriptor"/>
    <profile:hasRole rdf:resource="http://www.w3.org/ns/dx/prof/role/vocabulary"/>
    <dct:conformsTo rdf:resource="https://www.w3.org/TR/json-ld11/"/>
    <profile:hasArtifact rdf:resource="https://w3id.org/dpv/legal/de/gdng/de-gdng-owl.jsonld"/>
    <dct:format rdf:resource="https://www.iana.org/assignments/media-types/application/ld+json"/>
  </rdf:Description>
  <rdf:Description rdf:about="https://w3id.org/dpv/primer">
    <rdf:type rdf:resource="http://www.w3.org/ns/dx/prof/ResourceDescriptor"/>
    <dct:format rdf:resource="https://www.iana.org/assignments/media-types/text/html"/>
    <profile:hasRole rdf:resource="http://www.w3.org/ns/dx/prof/role/guidance"/>
    <dct:conformsTo rdf:resource="https://www.w3.org/TR/html/"/>
    <dct:title>Primer for Data Privacy Vocabulary</dct:title>
    <profile:hasArtifact rdf:resource="https://w3id.org/dpv/primer"/>
  </rdf:Description>
  <rdf:Description rdf:about="https://w3id.org/dpv/legal/de/gdng/owl#serialisation-rdf">
    <profile:hasArtifact rdf:resource="https://w3id.org/dpv/legal/de/gdng/de-gdng-owl.rdf"/>
    <dct:title>Legal Concepts for German Gesundheitsdatennutzungsgesetz (DE) - RDF/XML serialisation</dct:title>
    <dct:format rdf:resource="https://www.iana.org/assignments/media-types/application/rdf+xml"/>
    <profile:hasRole rdf:resource="http://www.w3.org/ns/dx/prof/role/vocabulary"/>
    <dct:conformsTo rdf:resource="http://www.w3.org/1999/02/22-rdf-syntax-ns#"/>
    <rdf:type rdf:resource="http://www.w3.org/ns/dx/prof/ResourceDescriptor"/>
  </rdf:Description>
  <rdf:Description rdf:about="https://w3id.org/dpv/legal/de/gdng/owl#DataProcessingHealthcareFacility">
    <rdfs:isDefinedBy rdf:resource="https://w3id.org/dpv/legal/de/gdng/owl#"/>
    <dct:created rdf:datatype="http://www.w3.org/2001/XMLSchema#date">2025-10-13</dct:created>
    <skos:prefLabel xml:lang="de">Datenverarbeitende Gesundheitseinrichtung</skos:prefLabel>
    <skos:prefLabel xml:lang="en">Data Processing Healthcare Facility</skos:prefLabel>
    <dct:contributor rdf:nodeID="person-julian-flake"/>
    <dct:contributor rdf:nodeID="person-christian-draeger"/>
    <dct:source xml:lang="en">[[GDNG]] § 2</dct:source>
    <rdf:type rdf:resource="http://www.w3.org/2000/01/rdf-schema#Class"/>
    <rdf:type rdf:resource="http://www.w3.org/2002/07/owl#Class"/>
    <sw:term_status xml:lang="en">accepted</sw:term_status>
    <skos:definition xml:lang="en">Institution which process data for the purposes of preventative or occupational medicine, for the assessment of the employee's capacity to work, for medical diagnosis, or for the purposes of care or treatment in the health or social sector under the responsibility of members of a health profession, where such a profession requires state-regulated training for the exercise of the profession or the use of the professional title</skos:definition>
    <skos:definition xml:lang="de">Einrichtung, in der für Zwecke der Gesundheitsvorsorge oder der Arbeitsmedizin, für die Beurteilung der Arbeitsfähigkeit des Beschäftigten, für die medizinische Diagnostik oder für Zwecke der Versorgung oder Behandlung im Gesundheits- oder Sozialbereich Daten von oder unter der Verantwortung von Angehörigen eines Heilberufs verarbeitet werden, der für die Berufsausübung oder die Führung der Berufsbezeichnung eine staatlich geregelte Ausbildung erfordert</skos:definition>
  </rdf:Description>
  <rdf:Description rdf:about="https://w3id.org/dpv/legal/de/gdng/owl#serialisation-n3">
    <dct:conformsTo rdf:resource="https://www.w3.org/TeamSubmission/n3/"/>
    <profile:hasRole rdf:resource="http://www.w3.org/ns/dx/prof/role/vocabulary"/>
    <rdf:type rdf:resource="http://www.w3.org/ns/dx/prof/ResourceDescriptor"/>
    <profile:hasArtifact rdf:resource="https://w3id.org/dpv/legal/de/gdng/de-gdng-owl.n3"/>
    <dct:title>Legal Concepts for German Gesundheitsdatennutzungsgesetz (DE) - N3 serialisation</dct:title>
    <dct:format rdf:resource="https://www.iana.org/assignments/media-types/text/n3"/>
  </rdf:Description>
  <rdf:Description rdf:nodeID="person-julian-flake">
    <org:memberOf rdf:nodeID="org-university-of-koblenz"/>
    <rdf:type rdf:resource="http://purl.org/dc/terms/Agent"/>
    <rdf:type rdf:resource="http://xmlns.com/foaf/0.1/Person"/>
    <scoro:hasORCID>0009-0006-4623-1463</scoro:hasORCID>
    <foaf:name>Julian Flake</foaf:name>
  </rdf:Description>
  <rdf:Description rdf:nodeID="org-university-of-leipzig">
    <rdf:type rdf:resource="http://xmlns.com/foaf/0.1/Organization"/>
    <foaf:name>University of Leipzig</foaf:name>
  </rdf:Description>
  <rdf:Description rdf:about="https://w3id.org/dpv/guides">
    <profile:hasArtifact rdf:resource="https://w3id.org/dpv/guides"/>
    <dct:format rdf:resource="https://www.iana.org/assignments/media-types/text/html"/>
    <profile:hasRole rdf:resource="http://www.w3.org/ns/dx/prof/role/guidance"/>
    <dct:conformsTo rdf:resource="https://www.w3.org/TR/html/"/>
    <rdf:type rdf:resource="http://www.w3.org/ns/dx/prof/ResourceDescriptor"/>
    <dct:title>Guides for Data Privacy Vocabulary</dct:title>
  </rdf:Description>
  <rdf:Description rdf:nodeID="person-christian-draeger">
    <org:memberOf rdf:nodeID="org-university-of-leipzig"/>
    <rdf:type rdf:resource="http://xmlns.com/foaf/0.1/Person"/>
    <rdf:type rdf:resource="http://purl.org/dc/terms/Agent"/>
    <foaf:name>Christian Draeger</foaf:name>
    <scoro:hasORCID>0000-0001-8835-4548</scoro:hasORCID>
  </rdf:Description>
</rdf:RDF>
