<?xml version="1.0" encoding="utf-8"?>
<rdf:RDF
   xmlns:bibo="http://purl.org/ontology/bibo/"
   xmlns:dct="http://purl.org/dc/terms/"
   xmlns:foaf="http://xmlns.com/foaf/0.1/"
   xmlns:org="http://www.w3.org/ns/org#"
   xmlns:owl="http://www.w3.org/2002/07/owl#"
   xmlns:profile="http://www.w3.org/ns/dx/prof/"
   xmlns:rdf="http://www.w3.org/1999/02/22-rdf-syntax-ns#"
   xmlns:rdfs="http://www.w3.org/2000/01/rdf-schema#"
   xmlns:schema="https://schema.org/"
   xmlns:scoro="http://purl.org/spar/scoro/"
   xmlns:skos="http://www.w3.org/2004/02/skos/core#"
   xmlns:sw="http://www.w3.org/2003/06/sw-vocab-status/ns#"
   xmlns:vann="http://purl.org/vocab/vann/"
>
  <rdf:Description rdf:about="https://w3id.org/dpv/legal/de/gdng#SecondaryUse">
    <sw:term_status xml:lang="en">accepted</sw:term_status>
    <rdf:type rdf:resource="http://www.w3.org/2004/02/skos/core#Concept"/>
    <rdf:type rdf:resource="http://www.w3.org/2000/01/rdf-schema#Class"/>
    <skos:prefLabel xml:lang="de">Sekundärdatennutzung</skos:prefLabel>
    <skos:prefLabel xml:lang="en">Secondary Use</skos:prefLabel>
    <skos:definition xml:lang="de">Weiterverarbeitung von Gesundheitsdaten zu anderen Zwecken als denjenigen, für die die Daten ursprünglich erhoben wurden</skos:definition>
    <skos:definition xml:lang="en">Processing of health data for purposes other than those for which the data was originally collected</skos:definition>
    <dct:source xml:lang="en">[[GDNG]] § 2 point 8</dct:source>
    <dct:contributor rdf:nodeID="person-julian-flake"/>
    <dct:created rdf:datatype="http://www.w3.org/2001/XMLSchema#date">2025-10-13</dct:created>
    <rdfs:isDefinedBy rdf:resource="https://w3id.org/dpv/legal/de/gdng#"/>
    <skos:inScheme rdf:resource="https://w3id.org/dpv/legal/de/gdng#basic-definitions-classes"/>
  </rdf:Description>
  <rdf:Description rdf:about="https://w3id.org/dpv/legal/de/gdng#serialisation-n3">
    <rdf:type rdf:resource="http://www.w3.org/ns/dx/prof/ResourceDescriptor"/>
    <profile:hasRole rdf:resource="http://www.w3.org/ns/dx/prof/role/vocabulary"/>
    <profile:hasArtifact rdf:resource="https://w3id.org/dpv/legal/de/gdng/de-gdng.n3"/>
    <dct:format rdf:resource="https://www.iana.org/assignments/media-types/text/n3"/>
    <dct:conformsTo rdf:resource="https://www.w3.org/TeamSubmission/n3/"/>
    <dct:title>Legal Concepts for German Gesundheitsdatennutzungsgesetz (DE) - N3 serialisation</dct:title>
  </rdf:Description>
  <rdf:Description rdf:about="https://w3id.org/dpv/examples">
    <rdf:type rdf:resource="http://www.w3.org/ns/dx/prof/ResourceDescriptor"/>
    <profile:hasRole rdf:resource="http://www.w3.org/ns/dx/prof/role/guidance"/>
    <profile:hasArtifact rdf:resource="https://w3id.org/dpv/examples"/>
    <dct:title>Examples</dct:title>
    <dct:format rdf:resource="https://www.iana.org/assignments/media-types/text/html"/>
    <dct:conformsTo rdf:resource="https://www.w3.org/TR/html/"/>
  </rdf:Description>
  <rdf:Description rdf:about="https://w3id.org/dpv/legal/de/gdng#HealthData">
    <sw:term_status xml:lang="en">accepted</sw:term_status>
    <rdf:type rdf:resource="http://www.w3.org/2004/02/skos/core#Concept"/>
    <rdf:type rdf:resource="http://www.w3.org/2000/01/rdf-schema#Class"/>
    <skos:prefLabel xml:lang="de">Gesundheitsdaten</skos:prefLabel>
    <skos:prefLabel xml:lang="en">Health Data</skos:prefLabel>
    <skos:definition xml:lang="de">Gesundheitdaten nach GDNG sind Gesundheitsdaten im Sinne des Artikels 4 Nummer 15 der DSGVO [[GDPR]], einschl. Gesundheitsdaten, die zugleich Sozialdaten nach § 67 des Zehnten Buches Sozialgesetzbuch sind</skos:definition>
    <skos:definition xml:lang="en">Health data according to GDNG follows the definition of health data of Art. 4 Nr. 15 [[GDPR]], including health data that is also social data according to § 67 of Zehntes Buch Sozialgesetzbuch</skos:definition>
    <dct:source xml:lang="en">[[GDNG]] § 2 point 1</dct:source>
    <dct:contributor rdf:nodeID="person-julian-flake"/>
    <dct:created rdf:datatype="http://www.w3.org/2001/XMLSchema#date">2025-10-13</dct:created>
    <rdfs:isDefinedBy rdf:resource="https://w3id.org/dpv/legal/de/gdng#"/>
    <skos:inScheme rdf:resource="https://w3id.org/dpv/legal/de/gdng#basic-definitions-classes"/>
  </rdf:Description>
  <rdf:Description rdf:nodeID="org-university-of-koblenz">
    <rdf:type rdf:resource="http://xmlns.com/foaf/0.1/Organization"/>
    <foaf:name>University of Koblenz</foaf:name>
  </rdf:Description>
  <rdf:Description rdf:about="https://w3id.org/dpv/legal/de/gdng">
    <rdf:type rdf:resource="http://www.w3.org/2002/07/owl#Ontology"/>
    <rdf:type rdf:resource="http://www.w3.org/ns/dx/prof/Profile"/>
    <owl:versionIRI rdf:resource="https://w3id.org/dpv/2.3/legal/de/gdng"/>
    <dct:source rdf:resource="https://www.w3.org/groups/cg/dpvcg/"/>
    <dct:title xml:lang="en">Legal Concepts for German Gesundheitsdatennutzungsgesetz (DE)</dct:title>
    <bibo:status>http://purl.org/ontology/bibo/status/draft</bibo:status>
    <rdfs:Label xml:lang="en">DE-GDNG</rdfs:Label>
    <dct:description xml:lang="en">Extension to the Data Privacy Vocabulary (DPV) providing concepts for representing legal information for a German regulation</dct:description>
    <dct:created xml:lang="en">2026-01-21</dct:created>
    <dct:issued xml:lang="en">2026-01-21</dct:issued>
    <dct:modified xml:lang="en">2026-02-25</dct:modified>
    <dct:creator rdf:nodeID="person-julian-flake"/>
    <dct:creator rdf:nodeID="person-christian-draeger"/>
    <schema:version>2.3</schema:version>
    <owl:versionInfo>2.3</owl:versionInfo>
    <dct:identifier>https://w3id.org/dpv/legal/de/gdng</dct:identifier>
    <dct:conformsTo>http://www.w3.org/2000/01/rdf-schema</dct:conformsTo>
    <dct:conformsTo>http://www.w3.org/2004/02/skos/core</dct:conformsTo>
    <bibo:doi>10.5281/zenodo.12505841</bibo:doi>
    <dct:bibliographicCitation>Harshvardhan J. Pandit, Beatriz Esteves, Georg P. Krog, Paul Ryan, Delaram Golpayegani, Julian Flake (2025) Data Privacy Vocabulary (DPV) – Version 2.0. In: Demartini, G., et al. The Semantic Web – ISWC 2024. ISWC 2024. Lecture Notes in Computer Science, vol 15233. Springer, Cham. https://doi.org/10.1007/978-3-031-77847-6_10</dct:bibliographicCitation>
    <dct:publisher rdf:resource="https://www.w3.org/"/>
    <foaf:logo rdf:resource="https://w3id.org/dpv/media/logo.png"/>
    <dct:contributor rdf:nodeID="person-julian-flake"/>
    <dct:license rdf:resource="https://www.w3.org/copyright/document-license-2023/"/>
    <vann:preferredNamespacePrefix>de-gdng</vann:preferredNamespacePrefix>
    <vann:preferredNamespaceUri>https://w3id.org/dpv/legal/de/gdng#</vann:preferredNamespaceUri>
    <profile:isProfileOf rdf:resource="http://www.w3.org/2000/01/rdf-schema#"/>
    <profile:isProfileOf rdf:resource="http://www.w3.org/2004/02/skos/core#"/>
    <profile:isProfileOf rdf:resource="https://w3id.org/dpv"/>
    <profile:hasResource rdf:resource="https://w3id.org/dpv/primer"/>
    <profile:hasResource rdf:resource="https://w3id.org/dpv/guides"/>
    <profile:hasResource rdf:resource="https://w3id.org/dpv/examples"/>
    <profile:hasResource rdf:resource="https://w3id.org/dpv/legal/de/gdng#serialisation-html"/>
    <profile:hasResource rdf:resource="https://w3id.org/dpv/legal/de/gdng#serialisation-rdf"/>
    <profile:hasResource rdf:resource="https://w3id.org/dpv/legal/de/gdng#serialisation-ttl"/>
    <profile:hasResource rdf:resource="https://w3id.org/dpv/legal/de/gdng#serialisation-n3"/>
    <profile:hasResource rdf:resource="https://w3id.org/dpv/legal/de/gdng#serialisation-jsonld"/>
  </rdf:Description>
  <rdf:Description rdf:about="https://w3id.org/dpv/legal/de/gdng#serialisation-jsonld">
    <rdf:type rdf:resource="http://www.w3.org/ns/dx/prof/ResourceDescriptor"/>
    <profile:hasRole rdf:resource="http://www.w3.org/ns/dx/prof/role/vocabulary"/>
    <profile:hasArtifact rdf:resource="https://w3id.org/dpv/legal/de/gdng/de-gdng.jsonld"/>
    <dct:format rdf:resource="https://www.iana.org/assignments/media-types/application/ld+json"/>
    <dct:conformsTo rdf:resource="https://www.w3.org/TR/json-ld11/"/>
    <dct:title>Legal Concepts for German Gesundheitsdatennutzungsgesetz (DE) - JSON-LD serialisation</dct:title>
  </rdf:Description>
  <rdf:Description rdf:about="https://w3id.org/dpv/legal/de/gdng#serialisation-rdf">
    <rdf:type rdf:resource="http://www.w3.org/ns/dx/prof/ResourceDescriptor"/>
    <profile:hasRole rdf:resource="http://www.w3.org/ns/dx/prof/role/vocabulary"/>
    <profile:hasArtifact rdf:resource="https://w3id.org/dpv/legal/de/gdng/de-gdng.rdf"/>
    <dct:format rdf:resource="https://www.iana.org/assignments/media-types/application/rdf+xml"/>
    <dct:conformsTo rdf:resource="http://www.w3.org/1999/02/22-rdf-syntax-ns#"/>
    <dct:title>Legal Concepts for German Gesundheitsdatennutzungsgesetz (DE) - RDF/XML serialisation</dct:title>
  </rdf:Description>
  <rdf:Description rdf:about="https://w3id.org/dpv/legal/de/gdng#serialisation-html">
    <rdf:type rdf:resource="http://www.w3.org/ns/dx/prof/ResourceDescriptor"/>
    <profile:hasRole rdf:resource="http://www.w3.org/ns/dx/prof/role/specification"/>
    <profile:hasArtifact rdf:resource="https://w3id.org/dpv/legal/de/gdng/de-gdng.html"/>
    <dct:format rdf:resource="https://www.iana.org/assignments/media-types/text/html"/>
    <dct:conformsTo rdf:resource="https://www.w3.org/TR/html/"/>
    <dct:title>Legal Concepts for German Gesundheitsdatennutzungsgesetz (DE) - HTML serialisation</dct:title>
  </rdf:Description>
  <rdf:Description rdf:about="https://w3id.org/dpv/legal/de/gdng#ResearchProject">
    <sw:term_status xml:lang="en">accepted</sw:term_status>
    <rdf:type rdf:resource="http://www.w3.org/2004/02/skos/core#Concept"/>
    <rdf:type rdf:resource="http://www.w3.org/2000/01/rdf-schema#Class"/>
    <skos:prefLabel xml:lang="de">Forschungsvorhaben</skos:prefLabel>
    <skos:prefLabel xml:lang="en">Research Project</skos:prefLabel>
    <skos:definition xml:lang="de">Ein Forschungsvorhaben im Sinne von Artikel 9 Absatz 2 Buchstabe j und Artikel 89 Absatz 1 Satz 1 und Absatz 2 der DSGVO [[GDPR]]</skos:definition>
    <skos:definition xml:lang="en">A research project in the sense of Art. 9(2)(j) and Art. 89(1), first sentence, and (2) [[GDPR]]</skos:definition>
    <dct:source xml:lang="en">[[GDNG]] § 2 point 5</dct:source>
    <dct:contributor rdf:nodeID="person-julian-flake"/>
    <dct:created rdf:datatype="http://www.w3.org/2001/XMLSchema#date">2025-10-13</dct:created>
    <rdfs:isDefinedBy rdf:resource="https://w3id.org/dpv/legal/de/gdng#"/>
    <skos:inScheme rdf:resource="https://w3id.org/dpv/legal/de/gdng#basic-definitions-classes"/>
  </rdf:Description>
  <rdf:Description rdf:about="https://w3id.org/dpv/legal/de/gdng#HealthAndHealthcareResearchProject">
    <sw:term_status xml:lang="en">accepted</sw:term_status>
    <rdf:type rdf:resource="http://www.w3.org/2004/02/skos/core#Concept"/>
    <rdf:type rdf:resource="http://www.w3.org/2000/01/rdf-schema#Class"/>
    <skos:prefLabel xml:lang="de">Gesundheits- und Versorgungsforschungsvorhaben</skos:prefLabel>
    <skos:prefLabel xml:lang="en">Health and Healthcare Research Project</skos:prefLabel>
    <skos:definition xml:lang="de">Forschungsvorhaben mit dem Ziel, die Gesundheit zu fördern, Krankheiten vorzubeugen, zu heilen und ihre Folgen zu vermindern, die Gesundheitsversorgung und -prävention zu verbessern sowie das Gesundheitswesen weiterzuentwickeln</skos:definition>
    <skos:definition xml:lang="en">Research project with the goal to promote health to prevent illnesses, to heal and to reduce their consequences, to improve health care and prevention and to develop healthcare system</skos:definition>
    <rdfs:subClassOf rdf:resource="https://w3id.org/dpv/legal/de/gdng#ResearchProject"/>
    <skos:broader rdf:resource="https://w3id.org/dpv/legal/de/gdng#ResearchProject"/>
    <dct:source xml:lang="en">[[GDNG]] § 2 point 6</dct:source>
    <dct:contributor rdf:nodeID="person-julian-flake"/>
    <dct:created rdf:datatype="http://www.w3.org/2001/XMLSchema#date">2025-10-13</dct:created>
    <rdfs:isDefinedBy rdf:resource="https://w3id.org/dpv/legal/de/gdng#"/>
    <skos:inScheme rdf:resource="https://w3id.org/dpv/legal/de/gdng#basic-definitions-classes"/>
  </rdf:Description>
  <rdf:Description rdf:about="https://w3id.org/dpv/legal/de/gdng#serialisation-ttl">
    <rdf:type rdf:resource="http://www.w3.org/ns/dx/prof/ResourceDescriptor"/>
    <profile:hasRole rdf:resource="http://www.w3.org/ns/dx/prof/role/vocabulary"/>
    <profile:hasArtifact rdf:resource="https://w3id.org/dpv/legal/de/gdng/de-gdng.ttl"/>
    <dct:format rdf:resource="https://www.iana.org/assignments/media-types/text/turtle"/>
    <dct:conformsTo rdf:resource="https://www.w3.org/TR/turtle/"/>
    <dct:title>Legal Concepts for German Gesundheitsdatennutzungsgesetz (DE) - Turtle serialisation</dct:title>
  </rdf:Description>
  <rdf:Description rdf:about="https://w3id.org/dpv/legal/de/gdng#basic-definitions-classes">
    <rdf:type rdf:resource="http://www.w3.org/2004/02/skos/core#ConceptScheme"/>
  </rdf:Description>
  <rdf:Description rdf:about="https://w3id.org/dpv/guides">
    <rdf:type rdf:resource="http://www.w3.org/ns/dx/prof/ResourceDescriptor"/>
    <profile:hasRole rdf:resource="http://www.w3.org/ns/dx/prof/role/guidance"/>
    <profile:hasArtifact rdf:resource="https://w3id.org/dpv/guides"/>
    <dct:title>Guides for Data Privacy Vocabulary</dct:title>
    <dct:format rdf:resource="https://www.iana.org/assignments/media-types/text/html"/>
    <dct:conformsTo rdf:resource="https://www.w3.org/TR/html/"/>
  </rdf:Description>
  <rdf:Description rdf:nodeID="person-christian-draeger">
    <rdf:type rdf:resource="http://xmlns.com/foaf/0.1/Person"/>
    <rdf:type rdf:resource="http://purl.org/dc/terms/Agent"/>
    <foaf:name>Christian Draeger</foaf:name>
    <scoro:hasORCID>0000-0001-8835-4548</scoro:hasORCID>
    <org:memberOf rdf:nodeID="org-university-of-leipzig"/>
  </rdf:Description>
  <rdf:Description rdf:nodeID="person-julian-flake">
    <rdf:type rdf:resource="http://xmlns.com/foaf/0.1/Person"/>
    <rdf:type rdf:resource="http://purl.org/dc/terms/Agent"/>
    <foaf:name>Julian Flake</foaf:name>
    <scoro:hasORCID>0009-0006-4623-1463</scoro:hasORCID>
    <org:memberOf rdf:nodeID="org-university-of-koblenz"/>
  </rdf:Description>
  <rdf:Description rdf:about="https://w3id.org/dpv/legal/de/gdng#PersonalData">
    <sw:term_status xml:lang="en">accepted</sw:term_status>
    <rdf:type rdf:resource="http://www.w3.org/2004/02/skos/core#Concept"/>
    <rdf:type rdf:resource="http://www.w3.org/2000/01/rdf-schema#Class"/>
    <skos:prefLabel xml:lang="de">Personenbezogene Daten</skos:prefLabel>
    <skos:prefLabel xml:lang="en">Personal Data</skos:prefLabel>
    <skos:definition xml:lang="de">Personenbezogene Daten nach GDNG sind personenbezogene Daten im Sinne von Artikel 4 der DSGVO [[GDPR]]</skos:definition>
    <skos:definition xml:lang="en">Persnal data in GDNG follows the definition of personal data of Art. 4 [[GDPR]]</skos:definition>
    <dct:source xml:lang="en">[[GDNG]] § 2 point 2</dct:source>
    <dct:contributor rdf:nodeID="person-julian-flake"/>
    <dct:created rdf:datatype="http://www.w3.org/2001/XMLSchema#date">2025-10-13</dct:created>
    <rdfs:isDefinedBy rdf:resource="https://w3id.org/dpv/legal/de/gdng#"/>
    <skos:inScheme rdf:resource="https://w3id.org/dpv/legal/de/gdng#basic-definitions-classes"/>
  </rdf:Description>
  <rdf:Description rdf:about="https://w3id.org/dpv/primer">
    <profile:hasRole rdf:resource="http://www.w3.org/ns/dx/prof/role/guidance"/>
    <rdf:type rdf:resource="http://www.w3.org/ns/dx/prof/ResourceDescriptor"/>
    <profile:hasArtifact rdf:resource="https://w3id.org/dpv/primer"/>
    <dct:title>Primer for Data Privacy Vocabulary</dct:title>
    <dct:format rdf:resource="https://www.iana.org/assignments/media-types/text/html"/>
    <dct:conformsTo rdf:resource="https://www.w3.org/TR/html/"/>
  </rdf:Description>
  <rdf:Description rdf:nodeID="org-university-of-leipzig">
    <rdf:type rdf:resource="http://xmlns.com/foaf/0.1/Organization"/>
    <foaf:name>University of Leipzig</foaf:name>
  </rdf:Description>
</rdf:RDF>
