<?xml version="1.0" encoding="utf-8"?>
<rdf:RDF
   xmlns:bibo="http://purl.org/ontology/bibo/"
   xmlns:dct="http://purl.org/dc/terms/"
   xmlns:foaf="http://xmlns.com/foaf/0.1/"
   xmlns:org="http://www.w3.org/ns/org#"
   xmlns:owl="http://www.w3.org/2002/07/owl#"
   xmlns:profile="http://www.w3.org/ns/dx/prof/"
   xmlns:rdf="http://www.w3.org/1999/02/22-rdf-syntax-ns#"
   xmlns:rdfs="http://www.w3.org/2000/01/rdf-schema#"
   xmlns:schema="https://schema.org/"
   xmlns:scoro="http://purl.org/spar/scoro/"
   xmlns:skos="http://www.w3.org/2004/02/skos/core#"
   xmlns:sw="http://www.w3.org/2003/06/sw-vocab-status/ns#"
   xmlns:vann="http://purl.org/vocab/vann/"
>
  <rdf:Description rdf:about="https://w3id.org/dpv/legal/de/gdng#HealthDataAccessApplication">
    <sw:term_status xml:lang="en">accepted</sw:term_status>
    <rdf:type rdf:resource="http://www.w3.org/2004/02/skos/core#Concept"/>
    <rdf:type rdf:resource="http://www.w3.org/2000/01/rdf-schema#Class"/>
    <skos:prefLabel xml:lang="de">Antrag auf Zugang zu Gesundheitsdaten</skos:prefLabel>
    <skos:prefLabel xml:lang="en">Health Data Access Application</skos:prefLabel>
    <skos:definition xml:lang="de">Prozess zur Beantragung von Zugang zu Gesundheitsdaten bei datenhaltenden Stellen durch Datennutzende, der durch die DACO unterstützt und koordiniert wird</skos:definition>
    <skos:definition xml:lang="en">Process of application by data users for access to health data stored at health data holders. The DACO supports data users with this process and coordinates communication</skos:definition>
    <dct:source xml:lang="en">[[GDNG]] § 3(2) point 3</dct:source>
    <dct:source xml:lang="en">4</dct:source>
    <dct:source xml:lang="en">5</dct:source>
    <dct:contributor rdf:nodeID="person-julian-flake"/>
    <dct:contributor rdf:nodeID="person-christian-henke"/>
    <dct:contributor rdf:nodeID="person-christian-draeger"/>
    <dct:created rdf:datatype="http://www.w3.org/2001/XMLSchema#date">2025-10-13</dct:created>
    <rdfs:isDefinedBy rdf:resource="https://w3id.org/dpv/legal/de/gdng#"/>
    <skos:inScheme rdf:resource="https://w3id.org/dpv/legal/de/gdng#query-and-access-classes"/>
  </rdf:Description>
  <rdf:Description rdf:about="https://w3id.org/dpv/legal/de/gdng#serialisation-n3">
    <rdf:type rdf:resource="http://www.w3.org/ns/dx/prof/ResourceDescriptor"/>
    <profile:hasRole rdf:resource="http://www.w3.org/ns/dx/prof/role/vocabulary"/>
    <profile:hasArtifact rdf:resource="https://w3id.org/dpv/legal/de/gdng/de-gdng.n3"/>
    <dct:format rdf:resource="https://www.iana.org/assignments/media-types/text/n3"/>
    <dct:conformsTo rdf:resource="https://www.w3.org/TeamSubmission/n3/"/>
    <dct:title>Legal Concepts for German Gesundheitsdatennutzungsgesetz (DE) - N3 serialisation</dct:title>
  </rdf:Description>
  <rdf:Description rdf:about="https://w3id.org/dpv/legal/de/gdng#HealthDataQuery">
    <sw:term_status xml:lang="en">accepted</sw:term_status>
    <rdf:type rdf:resource="http://www.w3.org/2004/02/skos/core#Concept"/>
    <rdf:type rdf:resource="http://www.w3.org/2000/01/rdf-schema#Class"/>
    <skos:prefLabel xml:lang="de">Identifizierung und Lokalisierung von Gesundheitsdaten</skos:prefLabel>
    <skos:prefLabel xml:lang="en">Indentification and Localization of Health Data</skos:prefLabel>
    <skos:definition xml:lang="de">Prozess der Identifizierung und Lokalisierung von Gesundheitsdaten durch Datennutzende für ihre Zwecke, welche dazu von der DACO beraten werden</skos:definition>
    <skos:definition xml:lang="en">Process of identification and localization of health data by health data users for their purposes, supported by the DACO</skos:definition>
    <dct:source xml:lang="en">[[GDNG]] § 3(2) point 2</dct:source>
    <dct:contributor rdf:nodeID="person-julian-flake"/>
    <dct:contributor rdf:nodeID="person-christian-henke"/>
    <dct:contributor rdf:nodeID="person-matthias-lobe"/>
    <dct:contributor rdf:nodeID="person-christian-draeger"/>
    <dct:created rdf:datatype="http://www.w3.org/2001/XMLSchema#date">2025-10-13</dct:created>
    <rdfs:isDefinedBy rdf:resource="https://w3id.org/dpv/legal/de/gdng#"/>
    <skos:inScheme rdf:resource="https://w3id.org/dpv/legal/de/gdng#query-and-access-classes"/>
  </rdf:Description>
  <rdf:Description rdf:about="https://w3id.org/dpv/examples">
    <rdf:type rdf:resource="http://www.w3.org/ns/dx/prof/ResourceDescriptor"/>
    <profile:hasRole rdf:resource="http://www.w3.org/ns/dx/prof/role/guidance"/>
    <profile:hasArtifact rdf:resource="https://w3id.org/dpv/examples"/>
    <dct:title>Examples</dct:title>
    <dct:format rdf:resource="https://www.iana.org/assignments/media-types/text/html"/>
    <dct:conformsTo rdf:resource="https://www.w3.org/TR/html/"/>
  </rdf:Description>
  <rdf:Description rdf:about="https://w3id.org/dpv/legal/de/gdng#HealthDataAccessApplicationRecord">
    <sw:term_status xml:lang="en">accepted</sw:term_status>
    <rdf:type rdf:resource="http://www.w3.org/2004/02/skos/core#Concept"/>
    <rdf:type rdf:resource="http://www.w3.org/2000/01/rdf-schema#Class"/>
    <skos:prefLabel xml:lang="de">Gesundheitsdatenzugangsantragsdaten</skos:prefLabel>
    <skos:prefLabel xml:lang="en">Health Data Access Application Record</skos:prefLabel>
    <skos:definition xml:lang="de">Im Rahmen der Antragsstellung des Zugangs auf Gesundheitsdaten zu erfassende und anfallende Daten, die auch im öffentlichen Antragsregister veröffentlicht werden</skos:definition>
    <skos:definition xml:lang="en">In course of health data access applications collected and produced data that is also published in the public health data access application register</skos:definition>
    <dct:source xml:lang="en">[[GDNG]] § 3(2) point 3</dct:source>
    <dct:source xml:lang="en">4</dct:source>
    <dct:source xml:lang="en">5</dct:source>
    <dct:source xml:lang="en">7</dct:source>
    <dct:contributor rdf:nodeID="person-julian-flake"/>
    <dct:contributor rdf:nodeID="person-christian-henke"/>
    <dct:contributor rdf:nodeID="person-christian-draeger"/>
    <dct:created rdf:datatype="http://www.w3.org/2001/XMLSchema#date">2026-02-09</dct:created>
    <rdfs:isDefinedBy rdf:resource="https://w3id.org/dpv/legal/de/gdng#"/>
    <skos:inScheme rdf:resource="https://w3id.org/dpv/legal/de/gdng#query-and-access-classes"/>
  </rdf:Description>
  <rdf:Description rdf:about="https://w3id.org/dpv/legal/de/gdng#SecureProcessingEnvironment">
    <sw:term_status xml:lang="en">accepted</sw:term_status>
    <rdf:type rdf:resource="http://www.w3.org/2004/02/skos/core#Concept"/>
    <rdf:type rdf:resource="http://www.w3.org/2000/01/rdf-schema#Class"/>
    <skos:prefLabel xml:lang="de">Sichere Verarbeitungsumgebung</skos:prefLabel>
    <skos:prefLabel xml:lang="en">Secure Processing Environment</skos:prefLabel>
    <skos:definition xml:lang="de">Durch die DACO konzeptionierte Maßnahme zur Verbesserung des Datenschutzes und der Datensicherheit im Rahmen der Weiterverarbeitung von Gesundheitsdaten zu Forschungszwecken und weiteren im Gemeinwohl liegenden Zwecken</skos:definition>
    <skos:definition xml:lang="en">A measure for improvement of data protection and information security in context of processing of health data for research purposes and common welfare, drafted by the DACO</skos:definition>
    <dct:source xml:lang="en">[[GDNG]] § 3(2) point 9</dct:source>
    <dct:contributor rdf:nodeID="person-julian-flake"/>
    <dct:contributor rdf:nodeID="person-christian-henke"/>
    <dct:created rdf:datatype="http://www.w3.org/2001/XMLSchema#date">2025-10-13</dct:created>
    <rdfs:isDefinedBy rdf:resource="https://w3id.org/dpv/legal/de/gdng#"/>
    <skos:inScheme rdf:resource="https://w3id.org/dpv/legal/de/gdng#query-and-access-classes"/>
  </rdf:Description>
  <rdf:Description rdf:nodeID="person-christian-henke">
    <rdf:type rdf:resource="http://xmlns.com/foaf/0.1/Person"/>
    <rdf:type rdf:resource="http://purl.org/dc/terms/Agent"/>
    <foaf:name>Christian Henke</foaf:name>
    <scoro:hasORCID>0000-0002-4541-4018</scoro:hasORCID>
    <org:memberOf rdf:nodeID="org-university-medical-center-gottingen"/>
  </rdf:Description>
  <rdf:Description rdf:about="https://w3id.org/dpv/legal/de/gdng#HealthDataQueryRecord">
    <sw:term_status xml:lang="en">accepted</sw:term_status>
    <rdf:type rdf:resource="http://www.w3.org/2004/02/skos/core#Concept"/>
    <rdf:type rdf:resource="http://www.w3.org/2000/01/rdf-schema#Class"/>
    <skos:prefLabel xml:lang="de">Gesundheitsdatenanfragedaten</skos:prefLabel>
    <skos:prefLabel xml:lang="en">Health Data Query Record</skos:prefLabel>
    <skos:definition xml:lang="de">Die im Rahmen der Identifikation und Lokalisierung von Gesundheitsdaten zu erfassenden und anfallende Daten</skos:definition>
    <skos:definition xml:lang="en">Data that is collected or produced during the identification and localization of health data</skos:definition>
    <dct:source xml:lang="en">[[GDNG]] § 3(2) point 2</dct:source>
    <dct:contributor rdf:nodeID="person-julian-flake"/>
    <dct:contributor rdf:nodeID="person-christian-henke"/>
    <dct:contributor rdf:nodeID="person-christian-draeger"/>
    <dct:created rdf:datatype="http://www.w3.org/2001/XMLSchema#date">2026-02-09</dct:created>
    <rdfs:isDefinedBy rdf:resource="https://w3id.org/dpv/legal/de/gdng#"/>
    <skos:inScheme rdf:resource="https://w3id.org/dpv/legal/de/gdng#query-and-access-classes"/>
  </rdf:Description>
  <rdf:Description rdf:nodeID="org-university-of-koblenz">
    <rdf:type rdf:resource="http://xmlns.com/foaf/0.1/Organization"/>
    <foaf:name>University of Koblenz</foaf:name>
  </rdf:Description>
  <rdf:Description rdf:about="https://w3id.org/dpv/legal/de/gdng">
    <rdf:type rdf:resource="http://www.w3.org/2002/07/owl#Ontology"/>
    <rdf:type rdf:resource="http://www.w3.org/ns/dx/prof/Profile"/>
    <owl:versionIRI rdf:resource="https://w3id.org/dpv/2.3/legal/de/gdng"/>
    <dct:source rdf:resource="https://www.w3.org/groups/cg/dpvcg/"/>
    <dct:title xml:lang="en">Legal Concepts for German Gesundheitsdatennutzungsgesetz (DE)</dct:title>
    <bibo:status>http://purl.org/ontology/bibo/status/draft</bibo:status>
    <rdfs:Label xml:lang="en">DE-GDNG</rdfs:Label>
    <dct:description xml:lang="en">Extension to the Data Privacy Vocabulary (DPV) providing concepts for representing legal information for a German regulation</dct:description>
    <dct:created xml:lang="en">2026-01-21</dct:created>
    <dct:issued xml:lang="en">2026-01-21</dct:issued>
    <dct:modified xml:lang="en">2026-02-25</dct:modified>
    <dct:creator rdf:nodeID="person-julian-flake"/>
    <dct:creator rdf:nodeID="person-christian-draeger"/>
    <schema:version>2.3</schema:version>
    <owl:versionInfo>2.3</owl:versionInfo>
    <dct:identifier>https://w3id.org/dpv/legal/de/gdng</dct:identifier>
    <dct:conformsTo>http://www.w3.org/2000/01/rdf-schema</dct:conformsTo>
    <dct:conformsTo>http://www.w3.org/2004/02/skos/core</dct:conformsTo>
    <bibo:doi>10.5281/zenodo.12505841</bibo:doi>
    <dct:bibliographicCitation>Harshvardhan J. Pandit, Beatriz Esteves, Georg P. Krog, Paul Ryan, Delaram Golpayegani, Julian Flake (2025) Data Privacy Vocabulary (DPV) – Version 2.0. In: Demartini, G., et al. The Semantic Web – ISWC 2024. ISWC 2024. Lecture Notes in Computer Science, vol 15233. Springer, Cham. https://doi.org/10.1007/978-3-031-77847-6_10</dct:bibliographicCitation>
    <dct:publisher rdf:resource="https://www.w3.org/"/>
    <foaf:logo rdf:resource="https://w3id.org/dpv/media/logo.png"/>
    <dct:contributor rdf:nodeID="person-matthias-lobe"/>
    <dct:contributor rdf:nodeID="person-julian-flake"/>
    <dct:contributor rdf:nodeID="person-christian-draeger"/>
    <dct:contributor rdf:nodeID="person-christian-henke"/>
    <dct:license rdf:resource="https://www.w3.org/copyright/document-license-2023/"/>
    <vann:preferredNamespacePrefix>de-gdng</vann:preferredNamespacePrefix>
    <vann:preferredNamespaceUri>https://w3id.org/dpv/legal/de/gdng#</vann:preferredNamespaceUri>
    <profile:isProfileOf rdf:resource="http://www.w3.org/2000/01/rdf-schema#"/>
    <profile:isProfileOf rdf:resource="http://www.w3.org/2004/02/skos/core#"/>
    <profile:isProfileOf rdf:resource="https://w3id.org/dpv"/>
    <profile:hasResource rdf:resource="https://w3id.org/dpv/primer"/>
    <profile:hasResource rdf:resource="https://w3id.org/dpv/guides"/>
    <profile:hasResource rdf:resource="https://w3id.org/dpv/examples"/>
    <profile:hasResource rdf:resource="https://w3id.org/dpv/legal/de/gdng#serialisation-html"/>
    <profile:hasResource rdf:resource="https://w3id.org/dpv/legal/de/gdng#serialisation-rdf"/>
    <profile:hasResource rdf:resource="https://w3id.org/dpv/legal/de/gdng#serialisation-ttl"/>
    <profile:hasResource rdf:resource="https://w3id.org/dpv/legal/de/gdng#serialisation-n3"/>
    <profile:hasResource rdf:resource="https://w3id.org/dpv/legal/de/gdng#serialisation-jsonld"/>
  </rdf:Description>
  <rdf:Description rdf:about="https://w3id.org/dpv/legal/de/gdng#serialisation-jsonld">
    <rdf:type rdf:resource="http://www.w3.org/ns/dx/prof/ResourceDescriptor"/>
    <profile:hasRole rdf:resource="http://www.w3.org/ns/dx/prof/role/vocabulary"/>
    <profile:hasArtifact rdf:resource="https://w3id.org/dpv/legal/de/gdng/de-gdng.jsonld"/>
    <dct:format rdf:resource="https://www.iana.org/assignments/media-types/application/ld+json"/>
    <dct:conformsTo rdf:resource="https://www.w3.org/TR/json-ld11/"/>
    <dct:title>Legal Concepts for German Gesundheitsdatennutzungsgesetz (DE) - JSON-LD serialisation</dct:title>
  </rdf:Description>
  <rdf:Description rdf:about="https://w3id.org/dpv/legal/de/gdng#query-and-access-classes">
    <rdf:type rdf:resource="http://www.w3.org/2004/02/skos/core#ConceptScheme"/>
  </rdf:Description>
  <rdf:Description rdf:about="https://w3id.org/dpv/legal/de/gdng#PublicHealthDataAccessApplicationRegister">
    <sw:term_status xml:lang="en">accepted</sw:term_status>
    <rdf:type rdf:resource="http://www.w3.org/2004/02/skos/core#Concept"/>
    <rdf:type rdf:resource="http://www.w3.org/2000/01/rdf-schema#Class"/>
    <skos:prefLabel xml:lang="de">Öffentliches Antragsregister</skos:prefLabel>
    <skos:prefLabel xml:lang="en">Public Health Data Access Application Register</skos:prefLabel>
    <skos:definition xml:lang="de">Von der DACO gepflegtes, öffentliches Register mit Informationen zu den über die DACO gestellten Anträgen auf Zugang zu Gesundheitsdaten, zu den Datennutzenden, zu den Vorhaben, für die Daten beantragt wurden, und zu deren Ergebnissen</skos:definition>
    <skos:definition xml:lang="en">A public registry of information about health data access applications, the corresponding data users, research projects and requested data, maintained by the DACO</skos:definition>
    <dct:source xml:lang="en">[[GDNG]] § 3(2) point7</dct:source>
    <dct:contributor rdf:nodeID="person-julian-flake"/>
    <dct:contributor rdf:nodeID="person-christian-henke"/>
    <dct:created rdf:datatype="http://www.w3.org/2001/XMLSchema#date">2025-10-13</dct:created>
    <rdfs:isDefinedBy rdf:resource="https://w3id.org/dpv/legal/de/gdng#"/>
    <skos:inScheme rdf:resource="https://w3id.org/dpv/legal/de/gdng#query-and-access-classes"/>
  </rdf:Description>
  <rdf:Description rdf:about="https://w3id.org/dpv/legal/de/gdng#serialisation-rdf">
    <rdf:type rdf:resource="http://www.w3.org/ns/dx/prof/ResourceDescriptor"/>
    <profile:hasRole rdf:resource="http://www.w3.org/ns/dx/prof/role/vocabulary"/>
    <profile:hasArtifact rdf:resource="https://w3id.org/dpv/legal/de/gdng/de-gdng.rdf"/>
    <dct:format rdf:resource="https://www.iana.org/assignments/media-types/application/rdf+xml"/>
    <dct:conformsTo rdf:resource="http://www.w3.org/1999/02/22-rdf-syntax-ns#"/>
    <dct:title>Legal Concepts for German Gesundheitsdatennutzungsgesetz (DE) - RDF/XML serialisation</dct:title>
  </rdf:Description>
  <rdf:Description rdf:about="https://w3id.org/dpv/legal/de/gdng#serialisation-html">
    <rdf:type rdf:resource="http://www.w3.org/ns/dx/prof/ResourceDescriptor"/>
    <profile:hasRole rdf:resource="http://www.w3.org/ns/dx/prof/role/specification"/>
    <profile:hasArtifact rdf:resource="https://w3id.org/dpv/legal/de/gdng/de-gdng.html"/>
    <dct:format rdf:resource="https://www.iana.org/assignments/media-types/text/html"/>
    <dct:conformsTo rdf:resource="https://www.w3.org/TR/html/"/>
    <dct:title>Legal Concepts for German Gesundheitsdatennutzungsgesetz (DE) - HTML serialisation</dct:title>
  </rdf:Description>
  <rdf:Description rdf:about="https://w3id.org/dpv/legal/de/gdng#PublicMetadataCatalogue">
    <sw:term_status xml:lang="en">accepted</sw:term_status>
    <rdf:type rdf:resource="http://www.w3.org/2004/02/skos/core#Concept"/>
    <rdf:type rdf:resource="http://www.w3.org/2000/01/rdf-schema#Class"/>
    <skos:prefLabel xml:lang="de">Öffentlicher Metadaten-Katalog</skos:prefLabel>
    <skos:prefLabel xml:lang="en">Public Metadata Catalogue</skos:prefLabel>
    <skos:definition xml:lang="de">Von der DACO barrierefrei zu führender und pflegender Katalog, in dem zu Transparenzzwecken Informationen über die im deutschen Gesundheitswesen vorhandenen und öffentlich zugänglichen Gesundheitsdaten und über die jeweiligen Halter dieser Daten gesammelt werden</skos:definition>
    <skos:definition xml:lang="en">An accessible catalog, driven and maintained by the DACO, in which information about existing and publicly available health data of the german health care along with the respective data holder are collected to fulfill transparency obligations</skos:definition>
    <dct:source xml:lang="en">[[GDNG]] § 3(2) point 1</dct:source>
    <dct:contributor rdf:nodeID="person-julian-flake"/>
    <dct:contributor rdf:nodeID="person-christian-henke"/>
    <dct:created rdf:datatype="http://www.w3.org/2001/XMLSchema#date">2025-10-13</dct:created>
    <rdfs:isDefinedBy rdf:resource="https://w3id.org/dpv/legal/de/gdng#"/>
    <skos:inScheme rdf:resource="https://w3id.org/dpv/legal/de/gdng#query-and-access-classes"/>
  </rdf:Description>
  <rdf:Description rdf:nodeID="person-matthias-lobe">
    <rdf:type rdf:resource="http://xmlns.com/foaf/0.1/Person"/>
    <rdf:type rdf:resource="http://purl.org/dc/terms/Agent"/>
    <foaf:name>Matthias Löbe</foaf:name>
    <scoro:hasORCID>0000-0002-2344-0426</scoro:hasORCID>
    <org:memberOf rdf:nodeID="org-university-of-leipzig"/>
  </rdf:Description>
  <rdf:Description rdf:about="https://w3id.org/dpv/legal/de/gdng#serialisation-ttl">
    <rdf:type rdf:resource="http://www.w3.org/ns/dx/prof/ResourceDescriptor"/>
    <profile:hasRole rdf:resource="http://www.w3.org/ns/dx/prof/role/vocabulary"/>
    <profile:hasArtifact rdf:resource="https://w3id.org/dpv/legal/de/gdng/de-gdng.ttl"/>
    <dct:format rdf:resource="https://www.iana.org/assignments/media-types/text/turtle"/>
    <dct:conformsTo rdf:resource="https://www.w3.org/TR/turtle/"/>
    <dct:title>Legal Concepts for German Gesundheitsdatennutzungsgesetz (DE) - Turtle serialisation</dct:title>
  </rdf:Description>
  <rdf:Description rdf:about="https://w3id.org/dpv/guides">
    <rdf:type rdf:resource="http://www.w3.org/ns/dx/prof/ResourceDescriptor"/>
    <profile:hasRole rdf:resource="http://www.w3.org/ns/dx/prof/role/guidance"/>
    <profile:hasArtifact rdf:resource="https://w3id.org/dpv/guides"/>
    <dct:title>Guides for Data Privacy Vocabulary</dct:title>
    <dct:format rdf:resource="https://www.iana.org/assignments/media-types/text/html"/>
    <dct:conformsTo rdf:resource="https://www.w3.org/TR/html/"/>
  </rdf:Description>
  <rdf:Description rdf:nodeID="person-christian-draeger">
    <rdf:type rdf:resource="http://xmlns.com/foaf/0.1/Person"/>
    <rdf:type rdf:resource="http://purl.org/dc/terms/Agent"/>
    <foaf:name>Christian Draeger</foaf:name>
    <scoro:hasORCID>0000-0001-8835-4548</scoro:hasORCID>
    <org:memberOf rdf:nodeID="org-university-of-leipzig"/>
  </rdf:Description>
  <rdf:Description rdf:nodeID="person-julian-flake">
    <rdf:type rdf:resource="http://xmlns.com/foaf/0.1/Person"/>
    <rdf:type rdf:resource="http://purl.org/dc/terms/Agent"/>
    <foaf:name>Julian Flake</foaf:name>
    <scoro:hasORCID>0009-0006-4623-1463</scoro:hasORCID>
    <org:memberOf rdf:nodeID="org-university-of-koblenz"/>
  </rdf:Description>
  <rdf:Description rdf:about="https://w3id.org/dpv/primer">
    <profile:hasRole rdf:resource="http://www.w3.org/ns/dx/prof/role/guidance"/>
    <rdf:type rdf:resource="http://www.w3.org/ns/dx/prof/ResourceDescriptor"/>
    <profile:hasArtifact rdf:resource="https://w3id.org/dpv/primer"/>
    <dct:title>Primer for Data Privacy Vocabulary</dct:title>
    <dct:format rdf:resource="https://www.iana.org/assignments/media-types/text/html"/>
    <dct:conformsTo rdf:resource="https://www.w3.org/TR/html/"/>
  </rdf:Description>
  <rdf:Description rdf:nodeID="org-university-medical-center-gottingen">
    <rdf:type rdf:resource="http://xmlns.com/foaf/0.1/Organization"/>
    <foaf:name>University Medical Center Göttingen</foaf:name>
  </rdf:Description>
  <rdf:Description rdf:nodeID="org-university-of-leipzig">
    <rdf:type rdf:resource="http://xmlns.com/foaf/0.1/Organization"/>
    <foaf:name>University of Leipzig</foaf:name>
  </rdf:Description>
</rdf:RDF>
