@prefix bibo: <http://purl.org/ontology/bibo/> .
@prefix dcam: <http://purl.org/dc/dcam/> .
@prefix dct: <http://purl.org/dc/terms/> .
@prefix dex: <https://w3id.org/dpv/examples#> .
@prefix dpv: <https://w3id.org/dpv#> .
@prefix foaf: <http://xmlns.com/foaf/0.1/> .
@prefix org: <http://www.w3.org/ns/org#> .
@prefix owl: <http://www.w3.org/2002/07/owl#> .
@prefix profile: <http://www.w3.org/ns/dx/prof/> .
@prefix rdf: <http://www.w3.org/1999/02/22-rdf-syntax-ns#> .
@prefix rdfs: <http://www.w3.org/2000/01/rdf-schema#> .
@prefix risk: <https://w3id.org/dpv/risk#> .
@prefix role: <http://www.w3.org/ns/dx/prof/role/> .
@prefix schema: <https://schema.org/> .
@prefix scoro: <http://purl.org/spar/scoro/> .
@prefix skos: <http://www.w3.org/2004/02/skos/core#> .
@prefix sw: <http://www.w3.org/2003/06/sw-vocab-status/ns#> .
@prefix vann: <http://purl.org/vocab/vann/> .
@prefix xsd: <http://www.w3.org/2001/XMLSchema#> .

risk:3LikelihoodLevels a rdfs:Class,
        skos:Concept,
        dpv:Likelihood ;
    dct:contributor _:person-harshvardhan-j-pandit ;
    dct:created "2022-08-18"^^xsd:date ;
    rdfs:isDefinedBy risk: ;
    sw:term_status "accepted"@en ;
    skos:broader dpv:Likelihood ;
    skos:definition "Scale with 3 Likelihood Levels from High to Low"@en ;
    skos:inScheme risk:risk-levels-classes ;
    skos:prefLabel "3 Likelihood Levels"@en .

risk:3RiskLevels a rdfs:Class,
        skos:Concept,
        dpv:RiskLevel ;
    dct:contributor _:person-harshvardhan-j-pandit ;
    dct:created "2022-08-18"^^xsd:date ;
    rdfs:isDefinedBy risk: ;
    sw:term_status "accepted"@en ;
    skos:broader dpv:RiskLevel ;
    skos:definition "Scale with 3 Risk Levels from High to Low"@en ;
    skos:inScheme risk:risk-levels-classes ;
    skos:prefLabel "3 Risk Levels"@en .

risk:3SeverityLevels a rdfs:Class,
        skos:Concept,
        dpv:Severity ;
    dct:contributor _:person-harshvardhan-j-pandit ;
    dct:created "2022-08-18"^^xsd:date ;
    rdfs:isDefinedBy risk: ;
    sw:term_status "accepted"@en ;
    skos:broader dpv:Severity ;
    skos:definition "Scale with 3 Severity Levels from High to Low"@en ;
    skos:inScheme risk:risk-levels-classes ;
    skos:prefLabel "3 Severity Levels"@en .

risk:5LikelihoodLevels a rdfs:Class,
        skos:Concept,
        dpv:Likelihood ;
    dct:contributor _:person-harshvardhan-j-pandit ;
    dct:created "2022-08-18"^^xsd:date ;
    rdfs:isDefinedBy risk: ;
    sw:term_status "accepted"@en ;
    skos:broader dpv:Likelihood ;
    skos:definition "Scale with 5 Likelihood Levels from Very High to Very Low"@en ;
    skos:inScheme risk:risk-levels-classes ;
    skos:prefLabel "5 Likelihood Levels"@en .

risk:5RiskLevels a rdfs:Class,
        skos:Concept,
        dpv:RiskLevel ;
    dct:contributor _:person-harshvardhan-j-pandit ;
    dct:created "2022-08-18"^^xsd:date ;
    rdfs:isDefinedBy risk: ;
    sw:term_status "accepted"@en ;
    skos:broader dpv:RiskLevel ;
    skos:definition "Scale with 5 Risk Levels from Very High to Very Low"@en ;
    skos:inScheme risk:risk-levels-classes ;
    skos:prefLabel "5 Risk Levels"@en .

risk:5SeverityLevels a rdfs:Class,
        skos:Concept,
        dpv:Severity ;
    dct:contributor _:person-harshvardhan-j-pandit ;
    dct:created "2022-08-18"^^xsd:date ;
    rdfs:isDefinedBy risk: ;
    sw:term_status "accepted"@en ;
    skos:broader dpv:Severity ;
    skos:definition "Scale with 5 Severity Levels from Very High to Very Low"@en ;
    skos:inScheme risk:risk-levels-classes ;
    skos:prefLabel "5 Severity Levels"@en .

risk:7LikelihoodLevels a rdfs:Class,
        skos:Concept,
        dpv:Likelihood ;
    dct:contributor _:person-harshvardhan-j-pandit ;
    dct:created "2022-08-18"^^xsd:date ;
    rdfs:isDefinedBy risk: ;
    sw:term_status "accepted"@en ;
    skos:broader dpv:Likelihood ;
    skos:definition "Scale with 7 Likelihood Levels from Extremely High to Extremely Low"@en ;
    skos:inScheme risk:risk-levels-classes ;
    skos:prefLabel "7 Likelihood Levels"@en .

risk:7RiskLevels a rdfs:Class,
        skos:Concept,
        dpv:RiskLevel ;
    dct:contributor _:person-harshvardhan-j-pandit ;
    dct:created "2022-08-18"^^xsd:date ;
    rdfs:isDefinedBy risk: ;
    sw:term_status "accepted"@en ;
    skos:broader dpv:RiskLevel ;
    skos:definition "Scale with 7 Risk Levels from Extremely High to Extremely Low"@en ;
    skos:inScheme risk:risk-levels-classes ;
    skos:prefLabel "7 Risk Levels"@en .

risk:7SeverityLevels a rdfs:Class,
        skos:Concept,
        dpv:Severity ;
    dct:contributor _:person-harshvardhan-j-pandit ;
    dct:created "2022-08-18"^^xsd:date ;
    rdfs:isDefinedBy risk: ;
    sw:term_status "accepted"@en ;
    skos:broader dpv:Severity ;
    skos:definition "Scale with 7 Severity Levels from Extremely High to Extremely Low"@en ;
    skos:inScheme risk:risk-levels-classes ;
    skos:prefLabel "7 Severity Levels"@en .

risk:AccidentalIncident a rdfs:Class,
        skos:Concept ;
    dct:created "2024-05-19"^^xsd:date ;
    rdfs:isDefinedBy risk: ;
    rdfs:subClassOf risk:Incident ;
    sw:term_status "accepted"@en ;
    skos:broader risk:Incident ;
    skos:definition "Incident caused due to accidental actions arising from human or human-controlled situations"@en ;
    skos:inScheme risk:incident-classes ;
    skos:prefLabel "Accidental Incident"@en .

risk:AccidentalMisuse a rdfs:Class,
        skos:Concept,
        dpv:RiskConcept,
        risk:PotentialConsequence,
        risk:PotentialRisk,
        risk:PotentialRiskSource ;
    dct:created "2024-12-17"^^xsd:date ;
    rdfs:isDefinedBy risk: ;
    sw:term_status "accepted"@en ;
    skos:broader risk:Misuse ;
    skos:definition "Concept representing accidental misuse (of something)"@en ;
    skos:inScheme risk:risk-taxonomy-classes ;
    skos:prefLabel "Accidental Misuse"@en .

risk:AccuracyDegraded a rdfs:Class,
        skos:Concept,
        dpv:RiskConcept,
        risk:PotentialConsequence,
        risk:PotentialRisk,
        risk:PotentialRiskSource ;
    dct:contributor _:person-delaram-golpayegani,
        _:person-harshvardhan-j-pandit ;
    dct:created "2024-12-01"^^xsd:date ;
    rdfs:isDefinedBy risk: ;
    sw:term_status "accepted"@en ;
    skos:broader risk:AccuracyRisk,
        risk:QualityDegraded ;
    skos:definition "Concepts representing risks and issues where Accuracy is Degraded"@en ;
    skos:inScheme risk:risk-taxonomy-classes ;
    skos:prefLabel "Accuracy Degraded"@en .

risk:AccuracyInconsistent a rdfs:Class,
        skos:Concept,
        dpv:RiskConcept,
        risk:PotentialConsequence,
        risk:PotentialRisk,
        risk:PotentialRiskSource ;
    dct:contributor _:person-harshvardhan-j-pandit ;
    dct:created "2024-12-01"^^xsd:date ;
    rdfs:isDefinedBy risk: ;
    sw:term_status "accepted"@en ;
    skos:broader risk:AccuracyRisk,
        risk:QualityInconsistent ;
    skos:definition "Concepts representing risks and issues where Accuracy is Inconsistent"@en ;
    skos:inScheme risk:risk-taxonomy-classes ;
    skos:prefLabel "Accuracy Inconsistent"@en .

risk:AccuracyInsufficient a rdfs:Class,
        skos:Concept,
        dpv:RiskConcept,
        risk:PotentialConsequence,
        risk:PotentialRisk,
        risk:PotentialRiskSource ;
    dct:contributor _:person-delaram-golpayegani,
        _:person-harshvardhan-j-pandit ;
    dct:created "2024-12-01"^^xsd:date ;
    rdfs:isDefinedBy risk: ;
    sw:term_status "accepted"@en ;
    skos:broader risk:AccuracyRisk,
        risk:QualityInsufficient ;
    skos:definition "Concepts representing risks and issues where Accuracy is Insufficient"@en ;
    skos:inScheme risk:risk-taxonomy-classes ;
    skos:prefLabel "Accuracy Insufficient"@en .

risk:AccuracyRisk a rdfs:Class,
        skos:Concept,
        dpv:RiskConcept,
        risk:PotentialConsequence,
        risk:PotentialRisk,
        risk:PotentialRiskSource ;
    dct:contributor _:person-harshvardhan-j-pandit ;
    dct:created "2024-12-01"^^xsd:date ;
    rdfs:isDefinedBy risk: ;
    sw:term_status "accepted"@en ;
    skos:broader risk:QualityRisk ;
    skos:definition "Concepts representing risks and issues where Accuracy is Risk"@en ;
    skos:inScheme risk:risk-taxonomy-classes ;
    skos:prefLabel "Accuracy Risk"@en .

risk:AccuracyUnknown a rdfs:Class,
        skos:Concept,
        dpv:RiskConcept,
        risk:PotentialConsequence,
        risk:PotentialRisk,
        risk:PotentialRiskSource ;
    dct:contributor _:person-harshvardhan-j-pandit ;
    dct:created "2024-12-01"^^xsd:date ;
    rdfs:isDefinedBy risk: ;
    sw:term_status "accepted"@en ;
    skos:broader risk:AccuracyRisk,
        risk:QualityUnknown ;
    skos:definition "Concepts representing risks and issues where Accuracy is Unknown"@en ;
    skos:inScheme risk:risk-taxonomy-classes ;
    skos:prefLabel "Accuracy Unknown"@en .

risk:AccuracyUnverified a rdfs:Class,
        skos:Concept,
        dpv:RiskConcept,
        risk:PotentialConsequence,
        risk:PotentialRisk,
        risk:PotentialRiskSource ;
    dct:contributor _:person-harshvardhan-j-pandit ;
    dct:created "2024-12-01"^^xsd:date ;
    rdfs:isDefinedBy risk: ;
    sw:term_status "accepted"@en ;
    skos:broader risk:AccuracyRisk,
        risk:QualityUnverified ;
    skos:definition "Concepts representing risks and issues where Accuracy is Unverified"@en ;
    skos:inScheme risk:risk-taxonomy-classes ;
    skos:prefLabel "Accuracy Unverified"@en .

risk:AgeDiscrimination a rdfs:Class,
        skos:Concept,
        dpv:RiskConcept,
        risk:PotentialConsequence,
        risk:PotentialImpact,
        risk:PotentialRisk ;
    dct:created "2024-09-30"^^xsd:date ;
    rdfs:isDefinedBy risk: ;
    sw:term_status "accepted"@en ;
    skos:broader risk:Discrimination ;
    skos:definition "Discrimination based on a person's age, often impacting older or younger individuals"@en ;
    skos:inScheme risk:risk-taxonomy-classes ;
    skos:prefLabel "Age Discrimination"@en .

risk:AuthorisationFailure a rdfs:Class,
        skos:Concept,
        dpv:RiskConcept,
        risk:ConfidentialityConcept,
        risk:IntegrityConcept,
        risk:PotentialRisk,
        risk:PotentialRiskSource ;
    dct:contributor _:person-harshvardhan-j-pandit ;
    dct:created "2022-08-17"^^xsd:date ;
    dct:modified "2024-08-16"^^xsd:date ;
    dct:source [ a schema:WebPage ;
            schema:name "ENISa Trust Services Security Incidents 2021" ;
            schema:url "https://www.enisa.europa.eu/publications/trust-services-security-incidents-2021" ] ;
    rdfs:isDefinedBy risk: ;
    sw:term_status "accepted"@en ;
    skos:broader risk:OperationalSecurityRisk ;
    skos:definition "Concept representing Authorisation Failure"@en ;
    skos:inScheme risk:risk-taxonomy-classes ;
    skos:prefLabel "Authorisation Failure"@en .

risk:AvailabilityBreach a rdfs:Class,
        skos:Concept,
        dpv:RiskConcept,
        risk:AvailabilityConcept,
        risk:PotentialConsequence,
        risk:PotentialRisk,
        risk:PotentialRiskSource ;
    dct:created "2024-12-17"^^xsd:date ;
    rdfs:isDefinedBy risk: ;
    sw:term_status "accepted"@en ;
    skos:broader risk:DataBreach ;
    skos:definition "Concept representing a breach of availability"@en ;
    skos:inScheme risk:risk-taxonomy-classes ;
    skos:prefLabel "Availability Breach"@en .

risk:AvailabilityConcept a rdfs:Class,
        skos:Concept ;
    dct:contributor _:person-harshvardhan-j-pandit ;
    dct:created "2024-09-29"^^xsd:date ;
    rdfs:isDefinedBy risk: ;
    rdfs:subClassOf dpv:RiskConcept ;
    sw:term_status "accepted"@en ;
    skos:broader dpv:RiskConcept ;
    skos:definition "Indicates a concept is relevant to 'Availability' in CIA InfoSec model"@en ;
    skos:inScheme risk:risk-taxonomy-classes ;
    skos:prefLabel "Availability Concept"@en ;
    skos:scopeNote "This concept allows indicating the applicability of Impact dimension to concepts whether they are a risk source, risk, consequence, or impact"@en .

risk:AvailabilityIncident a rdfs:Class,
        skos:Concept ;
    dct:created "2024-05-19"^^xsd:date ;
    rdfs:isDefinedBy risk: ;
    rdfs:subClassOf risk:Incident ;
    sw:term_status "accepted"@en ;
    skos:broader risk:Incident ;
    skos:definition "Incident where the availability of information or system has been affected"@en ;
    skos:inScheme risk:incident-classes ;
    skos:prefLabel "Availability Incident"@en .

risk:AvoidConsequence a rdfs:Class,
        skos:Concept,
        risk:RiskControl ;
    dct:contributor _:person-harshvardhan-j-pandit ;
    dct:created "2025-01-06"^^xsd:date ;
    rdfs:isDefinedBy risk: ;
    sw:term_status "accepted"@en ;
    skos:broader risk:AvoidanceControl,
        risk:ConsequenceControl ;
    skos:definition "Control that proactively avoids the consequence such that it has a reduced exposure or applicability in the context"@en ;
    skos:inScheme risk:risk-controls-classes ;
    skos:prefLabel "Avoid Consequence"@en .

risk:AvoidImpact a rdfs:Class,
        skos:Concept,
        risk:RiskControl ;
    dct:contributor _:person-harshvardhan-j-pandit ;
    dct:created "2025-01-06"^^xsd:date ;
    rdfs:isDefinedBy risk: ;
    sw:term_status "accepted"@en ;
    skos:broader risk:AvoidanceControl,
        risk:ImpactControl ;
    skos:definition "Control that proactively avoids the impact such that it has a reduced exposure or applicability in the context"@en ;
    skos:inScheme risk:risk-controls-classes ;
    skos:prefLabel "Avoid Impact"@en .

risk:AvoidSource a rdfs:Class,
        skos:Concept,
        risk:RiskControl ;
    dct:contributor _:person-harshvardhan-j-pandit ;
    dct:created "2024-05-19"^^xsd:date ;
    dct:modified "2025-01-06"^^xsd:date ;
    rdfs:isDefinedBy risk: ;
    sw:term_status "modified"@en ;
    skos:broader risk:AvoidanceControl,
        risk:SourceControl ;
    skos:definition "Control that proactively avoids the risk source such that it has a reduced exposure or applicability in the context"@en ;
    skos:inScheme risk:risk-controls-classes ;
    skos:prefLabel "Avoid Source"@en .

risk:AvoidanceControl a rdfs:Class,
        skos:Concept,
        risk:RiskControl ;
    dct:contributor _:person-harshvardhan-j-pandit ;
    dct:created "2025-01-06"^^xsd:date ;
    rdfs:isDefinedBy risk: ;
    sw:term_status "accepted"@en ;
    skos:broader risk:ProactiveControl ;
    skos:definition "Control that avoids an event with the goal of removing it completely"@en ;
    skos:inScheme risk:risk-controls-classes ;
    skos:prefLabel "Avoidance Control"@en ;
    skos:scopeNote "Avoiding is distinct from Mitigation and Modification as the goal to avoid an event is to prevent it from occurring at all, whereas mitigation and modification accept an event will occur and focus on managing it"@en .

risk:BehaviourDistortion a rdfs:Class,
        skos:Concept,
        dpv:RiskConcept,
        risk:PotentialConsequence,
        risk:PotentialImpact,
        risk:PotentialRisk ;
    dct:contributor _:person-delaram-golpayegani ;
    dct:created "2024-12-01"^^xsd:date ;
    rdfs:isDefinedBy risk: ;
    sw:term_status "accepted"@en ;
    skos:broader risk:IndividualRisk ;
    skos:definition "Concept representing distortion of behaviour of individual(s)"@en ;
    skos:inScheme risk:risk-taxonomy-classes ;
    skos:prefLabel "Behaviour Distortion"@en .

risk:BelievesDiscrimination a rdfs:Class,
        skos:Concept,
        dpv:RiskConcept,
        risk:PotentialConsequence,
        risk:PotentialImpact,
        risk:PotentialRisk ;
    dct:created "2024-09-30"^^xsd:date ;
    rdfs:isDefinedBy risk: ;
    sw:term_status "accepted"@en ;
    skos:broader risk:Discrimination ;
    skos:definition "Discrimination based on a person's beliefs or practices"@en ;
    skos:inScheme risk:risk-taxonomy-classes ;
    skos:prefLabel "Believes Discrimination"@en .

risk:Benefit a rdfs:Class,
        skos:Concept,
        dpv:RiskConcept,
        risk:PotentialConsequence,
        risk:PotentialImpact,
        risk:PotentialRisk ;
    dct:contributor _:person-axel-polleres,
        _:person-beatriz-esteves,
        _:person-fajar-ekaputra,
        _:person-georg-p-krog,
        _:person-harshvardhan-j-pandit,
        _:person-julian-flake ;
    dct:created "2022-03-23"^^xsd:date ;
    dct:modified "2024-08-16"^^xsd:date ;
    rdfs:isDefinedBy risk: ;
    sw:term_status "accepted"@en ;
    skos:broader risk:Compensation ;
    skos:definition "Concept representing benefits - both material and immaterial"@en ;
    skos:inScheme risk:risk-taxonomy-classes ;
    skos:prefLabel "Benefit"@en ;
    skos:scopeNote "Even though benefits is filed under organisational concepts, it can be applied to individuals (humans) and groups which are societal"@en .

risk:Bias a rdfs:Class,
        skos:Concept,
        dpv:RiskConcept,
        risk:PotentialConsequence,
        risk:PotentialRisk,
        risk:PotentialRiskSource ;
    dct:contributor _:person-daniel-doherty,
        _:person-delaram-golpayegani,
        _:person-harshvardhan-j-pandit ;
    dct:created "2024-09-13"^^xsd:date ;
    dct:source "ISO/IEC 24027:2021"@en ;
    rdfs:isDefinedBy risk: ;
    sw:term_status "accepted"@en ;
    skos:broader risk:TechnicalRiskConcept ;
    skos:definition "Bias is defined as the systematic difference in treatment of certain objects, people, or groups in comparison to others"@en ;
    skos:inScheme risk:risk-taxonomy-classes ;
    skos:prefLabel "Bias"@en .

risk:Blackmail a rdfs:Class,
        skos:Concept,
        dpv:RiskConcept,
        risk:ConfidentialityConcept,
        risk:PotentialConsequence,
        risk:PotentialRisk,
        risk:PotentialRiskSource ;
    dct:contributor _:person-harshvardhan-j-pandit ;
    dct:created "2022-08-17"^^xsd:date ;
    dct:modified "2026-02-09"^^xsd:date ;
    dct:source _:b15886bc6e88dcdb258fe59ded7be3abf ;
    rdfs:isDefinedBy risk: ;
    sw:term_status "modified"@en ;
    skos:broader risk:Exploitation ;
    skos:definition "Concept representing Blackmail"@en ;
    skos:inScheme risk:risk-taxonomy-classes ;
    skos:prefLabel "Blackmail"@en .

risk:BruteForceAuthorisations a rdfs:Class,
        skos:Concept,
        dpv:RiskConcept,
        risk:ConfidentialityConcept,
        risk:IntegrityConcept,
        risk:PotentialRisk,
        risk:PotentialRiskSource ;
    dct:contributor _:person-harshvardhan-j-pandit ;
    dct:created "2022-08-17"^^xsd:date ;
    dct:modified "2024-08-16"^^xsd:date ;
    dct:source _:b7191aa21b975cb14bbce32aa3ba9c7eb ;
    rdfs:isDefinedBy risk: ;
    sw:term_status "accepted"@en ;
    skos:broader risk:SecurityAttack ;
    skos:definition "Concept representing Brute Force Authorisations i.e. bypassing authorisations through brute forcing techniques"@en ;
    skos:inScheme risk:risk-taxonomy-classes ;
    skos:prefLabel "Brute Force Authorisations"@en .

risk:CasteDiscrimination a rdfs:Class,
        skos:Concept,
        dpv:RiskConcept,
        risk:PotentialConsequence,
        risk:PotentialImpact,
        risk:PotentialRisk ;
    dct:created "2024-09-30"^^xsd:date ;
    rdfs:isDefinedBy risk: ;
    sw:term_status "accepted"@en ;
    skos:broader risk:Discrimination ;
    skos:definition "Discrimination based on a person's caste, a form of social stratification found in some cultures"@en ;
    skos:inScheme risk:risk-taxonomy-classes ;
    skos:prefLabel "Caste Discrimination"@en .

risk:ChangeConsequence a rdfs:Class,
        skos:Concept,
        risk:RiskControl ;
    dct:contributor _:person-harshvardhan-j-pandit ;
    dct:created "2024-05-19"^^xsd:date ;
    dct:modified "2025-01-06"^^xsd:date ;
    rdfs:isDefinedBy risk: ;
    sw:term_status "modified"@en ;
    skos:broader risk:ConsequenceControl,
        risk:SubstitutionControl ;
    skos:definition "Control that proactively changes the consequence event such that one event is replaced with the occurrence or applicability of another event in the context"@en ;
    skos:inScheme risk:risk-controls-classes ;
    skos:prefLabel "Change Consequence"@en .

risk:ChangeImpact a rdfs:Class,
        skos:Concept,
        risk:RiskControl ;
    dct:contributor _:person-harshvardhan-j-pandit ;
    dct:created "2024-05-19"^^xsd:date ;
    dct:modified "2025-01-06"^^xsd:date ;
    rdfs:isDefinedBy risk: ;
    sw:term_status "modified"@en ;
    skos:broader risk:ImpactControl,
        risk:SubstitutionControl ;
    skos:definition "Control that proactively changes the impact event such that one event is replaced with the occurrence or applicability of another event in the context"@en ;
    skos:inScheme risk:risk-controls-classes ;
    skos:prefLabel "Change Impact"@en .

risk:Coercion a rdfs:Class,
        skos:Concept,
        dpv:RiskConcept,
        risk:ConfidentialityConcept,
        risk:PotentialConsequence,
        risk:PotentialRisk,
        risk:PotentialRiskSource ;
    dct:contributor _:person-harshvardhan-j-pandit ;
    dct:created "2022-08-17"^^xsd:date ;
    dct:modified "2024-08-16"^^xsd:date ;
    dct:source _:b65de0d403668931587d7f38d790f5adc ;
    rdfs:isDefinedBy risk: ;
    sw:term_status "accepted"@en ;
    skos:broader risk:Exploitation ;
    skos:definition "Concept representing Coercion"@en ;
    skos:inScheme risk:risk-taxonomy-classes ;
    skos:prefLabel "Coercion"@en .

risk:CognitiveBias a rdfs:Class,
        skos:Concept,
        dpv:RiskConcept,
        risk:PotentialConsequence,
        risk:PotentialRisk,
        risk:PotentialRiskSource ;
    dct:contributor _:person-daniel-doherty,
        _:person-delaram-golpayegani,
        _:person-harshvardhan-j-pandit ;
    dct:created "2024-09-13"^^xsd:date ;
    dct:source "ISO/IEC 24027:2021"@en ;
    rdfs:isDefinedBy risk: ;
    sw:term_status "accepted"@en ;
    skos:broader risk:Bias ;
    skos:definition "Bias that occurs when humans are processing and interpreting information"@en ;
    skos:inScheme risk:risk-taxonomy-classes ;
    skos:prefLabel "Cognitive Bias"@en .

risk:Compensation a rdfs:Class,
        skos:Concept,
        dpv:RiskConcept,
        risk:PotentialConsequence,
        risk:PotentialImpact,
        risk:PotentialRisk ;
    dct:contributor _:person-georg-p-krog,
        _:person-harshvardhan-j-pandit ;
    dct:created "2024-04-14"^^xsd:date ;
    dct:modified "2025-08-06"^^xsd:date ;
    rdfs:isDefinedBy risk: ;
    sw:term_status "modified"@en ;
    skos:broader risk:Remuneration ;
    skos:definition "Something that acts as or provides compensation - which can be monetary and financial or in other forms"@en ;
    skos:inScheme risk:risk-taxonomy-classes ;
    skos:prefLabel "Compensation"@en .

risk:ComponentFailure a rdfs:Class,
        skos:Concept,
        dpv:RiskConcept,
        risk:AvailabilityConcept,
        risk:PotentialConsequence,
        risk:PotentialRisk,
        risk:PotentialRiskSource ;
    dct:contributor _:person-delaram-golpayegani ;
    dct:created "2024-12-01"^^xsd:date ;
    rdfs:isDefinedBy risk: ;
    sw:term_status "accepted"@en ;
    skos:broader risk:OperationalSecurityRisk ;
    skos:definition "Concept representing Component Failure"@en ;
    skos:inScheme risk:risk-taxonomy-classes ;
    skos:prefLabel "Component Failure"@en ;
    skos:scopeNote "Here component refers to both physical and virtual components. The failure of a component may or may not also cause a failure in other related components or the systems they are part of"@en .

risk:ComponentMalfunction a rdfs:Class,
        skos:Concept,
        dpv:RiskConcept,
        risk:AvailabilityConcept,
        risk:PotentialConsequence,
        risk:PotentialRisk,
        risk:PotentialRiskSource ;
    dct:contributor _:person-delaram-golpayegani ;
    dct:created "2024-12-01"^^xsd:date ;
    rdfs:isDefinedBy risk: ;
    sw:term_status "accepted"@en ;
    skos:broader risk:OperationalSecurityRisk ;
    skos:definition "Concept representing Component Malfunction"@en ;
    skos:inScheme risk:risk-taxonomy-classes ;
    skos:prefLabel "Component Malfunction"@en ;
    skos:scopeNote "Here component refers to both physical and virtual components. The malfunction of a component may or may not also cause a malfunction in other related components or the systems they are part of"@en .

risk:CompromiseAccount a rdfs:Class,
        skos:Concept,
        dpv:RiskConcept,
        risk:AvailabilityConcept,
        risk:ConfidentialityConcept,
        risk:IntegrityConcept,
        risk:PotentialConsequence,
        risk:PotentialRisk,
        risk:PotentialRiskSource ;
    dct:contributor _:person-harshvardhan-j-pandit ;
    dct:created "2022-08-17"^^xsd:date ;
    dct:modified "2024-08-16"^^xsd:date ;
    dct:source _:b7191aa21b975cb14bbce32aa3ba9c7eb ;
    rdfs:isDefinedBy risk: ;
    sw:term_status "accepted"@en ;
    skos:broader risk:ExternalSecurityThreat ;
    skos:definition "Concept representing a compromised account that is then used by the compromiser"@en ;
    skos:inScheme risk:risk-taxonomy-classes ;
    skos:prefLabel "Compromise Account"@en .

risk:CompromiseAccountCredentials a rdfs:Class,
        skos:Concept,
        dpv:RiskConcept,
        risk:ConfidentialityConcept,
        risk:PotentialConsequence,
        risk:PotentialRisk,
        risk:PotentialRiskSource ;
    dct:contributor _:person-harshvardhan-j-pandit ;
    dct:created "2022-08-17"^^xsd:date ;
    dct:modified "2024-08-16"^^xsd:date ;
    dct:source _:b7191aa21b975cb14bbce32aa3ba9c7eb ;
    rdfs:isDefinedBy risk: ;
    sw:term_status "accepted"@en ;
    skos:broader risk:ExternalSecurityThreat ;
    skos:definition "Concept representing Account Credentials to be compromised"@en ;
    skos:inScheme risk:risk-taxonomy-classes ;
    skos:prefLabel "Compromise Account Credentials"@en .

risk:ConfidentialityBreach a rdfs:Class,
        skos:Concept,
        dpv:RiskConcept,
        risk:ConfidentialityConcept,
        risk:PotentialConsequence,
        risk:PotentialRisk,
        risk:PotentialRiskSource ;
    dct:contributor _:person-harshvardhan-j-pandit ;
    dct:created "2022-08-17"^^xsd:date ;
    dct:modified "2024-08-16"^^xsd:date ;
    dct:source _:b15886bc6e88dcdb258fe59ded7be3abf ;
    rdfs:isDefinedBy risk: ;
    sw:term_status "accepted"@en ;
    skos:broader risk:DataBreach ;
    skos:definition "Concept representing a breach of confidentiality"@en ;
    skos:inScheme risk:risk-taxonomy-classes ;
    skos:prefLabel "Confidentiality Breach"@en .

risk:ConfidentialityConcept a rdfs:Class,
        skos:Concept ;
    dct:contributor _:person-harshvardhan-j-pandit ;
    dct:created "2024-09-29"^^xsd:date ;
    rdfs:isDefinedBy risk: ;
    rdfs:subClassOf dpv:RiskConcept ;
    sw:term_status "accepted"@en ;
    skos:broader dpv:RiskConcept ;
    skos:definition "Indicates a concept is relevant to 'Confidentiality' in CIA InfoSec model"@en ;
    skos:inScheme risk:risk-taxonomy-classes ;
    skos:prefLabel "Confidentiality Concept"@en ;
    skos:scopeNote "This concept allows indicating the applicability of Confidentiality dimension to concepts whether they are a risk source, risk, consequence, or impact"@en .

risk:ConfidentialityIncident a rdfs:Class,
        skos:Concept ;
    dct:created "2024-05-19"^^xsd:date ;
    rdfs:isDefinedBy risk: ;
    rdfs:subClassOf risk:Incident ;
    sw:term_status "accepted"@en ;
    skos:broader risk:Incident ;
    skos:definition "Incident where the confidentiality of information or system has been affected"@en ;
    skos:inScheme risk:incident-classes ;
    skos:prefLabel "Confidentiality Incident"@en .

risk:ConfirmationBias a rdfs:Class,
        skos:Concept,
        dpv:RiskConcept,
        risk:PotentialConsequence,
        risk:PotentialRisk,
        risk:PotentialRiskSource ;
    dct:contributor _:person-daniel-doherty,
        _:person-delaram-golpayegani,
        _:person-harshvardhan-j-pandit ;
    dct:created "2024-09-13"^^xsd:date ;
    dct:source "ISO/IEC 24027:2021"@en ;
    rdfs:isDefinedBy risk: ;
    sw:term_status "accepted"@en ;
    skos:broader risk:CognitiveBias ;
    skos:definition "Bias that occurs when hypotheses, regardless of their veracity, are more likely to be confirmed by the intentional or unintentional interpretation of information"@en ;
    skos:inScheme risk:risk-taxonomy-classes ;
    skos:prefLabel "Confirmation Bias"@en .

risk:ConfoundingVariablesBias a rdfs:Class,
        skos:Concept,
        dpv:RiskConcept,
        risk:PotentialConsequence,
        risk:PotentialRisk,
        risk:PotentialRiskSource ;
    dct:contributor _:person-daniel-doherty,
        _:person-delaram-golpayegani,
        _:person-harshvardhan-j-pandit ;
    dct:created "2024-09-13"^^xsd:date ;
    dct:source "ISO/IEC 24027:2021"@en ;
    rdfs:isDefinedBy risk: ;
    sw:term_status "accepted"@en ;
    skos:broader risk:StatisticalBias ;
    skos:definition "Bias that occurs as a confounding variable that influences both the dependent variable and independent variable causing a spurious association"@en ;
    skos:inScheme risk:risk-taxonomy-classes ;
    skos:prefLabel "Confounding Variables Bias"@en .

risk:ConsequenceControl a rdfs:Class,
        skos:Concept,
        risk:RiskControl ;
    dct:contributor _:person-harshvardhan-j-pandit ;
    dct:created "2024-05-19"^^xsd:date ;
    dct:modified "2025-01-06"^^xsd:date ;
    rdfs:isDefinedBy risk: ;
    sw:term_status "modified"@en ;
    skos:broader risk:RiskControl ;
    skos:definition "Risk control for managing consequences"@en ;
    skos:inScheme risk:risk-controls-classes ;
    skos:prefLabel "Consequence Control"@en .

risk:ContainmentControl a rdfs:Class,
        skos:Concept,
        risk:RiskControl ;
    dct:contributor _:person-delaram-golpayegani,
        _:person-harshvardhan-j-pandit ;
    dct:created "2024-05-19"^^xsd:date ;
    dct:modified "2025-01-06"^^xsd:date ;
    rdfs:isDefinedBy risk: ;
    sw:term_status "modified"@en ;
    skos:broader risk:ReductionControl ;
    skos:definition "Control that aims to contain the event in terms of limiting its occurrence or effects"@en ;
    skos:inScheme risk:risk-controls-classes ;
    skos:prefLabel "Containment Control"@en ;
    skos:scopeNote "Containment implies either changing the event or the context such that the event's effects are restricted, such as by establishing a physical or digital boundary within which the effects can occur or to prevent the effects from affecting things inside the boundary"@en .

risk:CopyrightViolation a rdfs:Class,
        skos:Concept,
        dpv:RiskConcept,
        risk:PotentialConsequence,
        risk:PotentialRisk ;
    dct:contributor _:person-harshvardhan-j-pandit ;
    dct:created "2022-08-17"^^xsd:date ;
    dct:modified "2024-08-16"^^xsd:date ;
    dct:source _:b7191aa21b975cb14bbce32aa3ba9c7eb ;
    rdfs:isDefinedBy risk: ;
    sw:term_status "accepted"@en ;
    skos:broader risk:LegalComplianceRisk,
        risk:ViolatingObligation ;
    skos:definition "Concept representing Copyright Violation"@en ;
    skos:inScheme risk:risk-taxonomy-classes ;
    skos:prefLabel "Copyright Violation"@en .

risk:CoverageBias a rdfs:Class,
        skos:Concept,
        dpv:RiskConcept,
        risk:PotentialConsequence,
        risk:PotentialRisk,
        risk:PotentialRiskSource ;
    dct:contributor _:person-daniel-doherty,
        _:person-delaram-golpayegani,
        _:person-harshvardhan-j-pandit ;
    dct:created "2024-09-13"^^xsd:date ;
    dct:source "ISO/IEC 24027:2021"@en ;
    rdfs:isDefinedBy risk: ;
    sw:term_status "accepted"@en ;
    skos:broader risk:SelectionBias ;
    skos:definition "Bias that occurs when a population represented in a dataset does not match the actual or real population that are being used"@en ;
    skos:inScheme risk:risk-taxonomy-classes ;
    skos:prefLabel "Coverage Bias"@en .

risk:CredibilityLoss a rdfs:Class,
        skos:Concept,
        dpv:RiskConcept,
        risk:PotentialConsequence,
        risk:PotentialImpact,
        risk:PotentialRisk ;
    dct:contributor _:person-harshvardhan-j-pandit ;
    dct:created "2022-08-17"^^xsd:date ;
    dct:modified "2025-08-24"^^xsd:date ;
    dct:source _:b15886bc6e88dcdb258fe59ded7be3abf ;
    rdfs:isDefinedBy risk: ;
    sw:term_status "modified"@en ;
    skos:broader risk:ReputationalRisk ;
    skos:definition "Concept representing Credibility Loss"@en ;
    skos:inScheme risk:risk-taxonomy-classes ;
    skos:prefLabel "Credibility Loss"@en .

risk:CrossBorderIncident a rdfs:Class,
        skos:Concept ;
    dct:created "2024-05-19"^^xsd:date ;
    rdfs:isDefinedBy risk: ;
    rdfs:subClassOf risk:Incident ;
    sw:term_status "accepted"@en ;
    skos:broader risk:Incident ;
    skos:definition "Incident involving cross-border or multiple jurisdictions"@en ;
    skos:inScheme risk:incident-classes ;
    skos:prefLabel "Cross-Border Incident"@en .

risk:Cryptojacking a rdfs:Class,
        skos:Concept,
        dpv:RiskConcept,
        risk:AvailabilityConcept,
        risk:PotentialRisk,
        risk:PotentialRiskSource ;
    dct:contributor _:person-harshvardhan-j-pandit ;
    dct:created "2022-08-17"^^xsd:date ;
    dct:modified "2024-08-16"^^xsd:date ;
    dct:source [ a schema:WebPage ;
            schema:name "ENISA Threat Landscape 2021" ;
            schema:url "https://www.enisa.europa.eu/publications/enisa-threat-landscape-2021" ] ;
    rdfs:isDefinedBy risk: ;
    sw:term_status "accepted"@en ;
    skos:broader risk:SecurityAttack ;
    skos:definition "Concept representing Cryptojacking"@en ;
    skos:inScheme risk:risk-taxonomy-classes ;
    skos:prefLabel "Cryptojacking"@en .

risk:CustomerConfidenceLoss a rdfs:Class,
        skos:Concept,
        dpv:RiskConcept,
        risk:PotentialConsequence,
        risk:PotentialImpact,
        risk:PotentialRisk ;
    dct:contributor _:person-harshvardhan-j-pandit ;
    dct:created "2022-08-17"^^xsd:date ;
    dct:modified "2025-08-24"^^xsd:date ;
    dct:source _:b15886bc6e88dcdb258fe59ded7be3abf ;
    rdfs:isDefinedBy risk: ;
    sw:term_status "modified"@en ;
    skos:broader risk:ReputationalRisk ;
    skos:definition "Concept representing Customer Confidence Loss"@en ;
    skos:inScheme risk:risk-taxonomy-classes ;
    skos:prefLabel "Customer Confidence Loss"@en .

risk:CustomerSupportLimited a rdfs:Class,
        skos:Concept,
        dpv:RiskConcept,
        risk:PotentialConsequence,
        risk:PotentialImpact,
        risk:PotentialRisk ;
    dct:created "2024-10-21"^^xsd:date ;
    rdfs:isDefinedBy risk: ;
    sw:term_status "accepted"@en ;
    skos:broader risk:ServiceRelatedConsequence ;
    skos:definition "Concept representing customer support to be limited"@en ;
    skos:inScheme risk:risk-taxonomy-classes ;
    skos:prefLabel "Customer Support Limited"@en .

risk:Damage a rdfs:Class,
        skos:Concept,
        dpv:RiskConcept,
        risk:PotentialConsequence,
        risk:PotentialImpact,
        risk:PotentialRisk ;
    dct:contributor _:person-harshvardhan-j-pandit ;
    dct:created "2022-03-30"^^xsd:date ;
    dct:modified "2024-08-16"^^xsd:date ;
    rdfs:isDefinedBy risk: ;
    sw:term_status "accepted"@en ;
    skos:broader risk:LegallyRelevantConsequence ;
    skos:definition "Concept representing Damage"@en ;
    skos:inScheme risk:risk-taxonomy-classes ;
    skos:prefLabel "Damage"@en .

risk:DataAggregationBias a rdfs:Class,
        skos:Concept,
        dpv:RiskConcept,
        risk:PotentialConsequence,
        risk:PotentialRisk,
        risk:PotentialRiskSource ;
    dct:contributor _:person-daniel-doherty,
        _:person-delaram-golpayegani,
        _:person-harshvardhan-j-pandit ;
    dct:created "2024-09-13"^^xsd:date ;
    dct:source "ISO/IEC 24027:2021"@en ;
    rdfs:isDefinedBy risk: ;
    sw:term_status "accepted"@en ;
    skos:broader risk:DataBias ;
    skos:definition "Bias that occurs when aggregating data covering different groups of objects has different statistical distributions that introduce bias into the data"@en ;
    skos:inScheme risk:risk-taxonomy-classes ;
    skos:prefLabel "Data Aggregation Bias"@en .

risk:DataBias a rdfs:Class,
        skos:Concept,
        dpv:RiskConcept,
        risk:PotentialConsequence,
        risk:PotentialRisk,
        risk:PotentialRiskSource ;
    dct:contributor _:person-daniel-doherty,
        _:person-delaram-golpayegani,
        _:person-harshvardhan-j-pandit ;
    dct:created "2024-09-13"^^xsd:date ;
    dct:source "ISO/IEC 24027:2021"@en ;
    rdfs:isDefinedBy risk: ;
    sw:term_status "accepted"@en ;
    skos:broader risk:Bias,
        risk:DataRisk ;
    skos:definition "Bias that occurs when data properties that if unaddressed lead to systems that perform better or worse for different groups"@en ;
    skos:inScheme risk:risk-taxonomy-classes ;
    skos:prefLabel "Data Bias"@en .

risk:DataBreach a rdfs:Class,
        skos:Concept,
        dpv:RiskConcept,
        risk:AvailabilityConcept,
        risk:ConfidentialityConcept,
        risk:IntegrityConcept,
        risk:PotentialConsequence,
        risk:PotentialRisk,
        risk:PotentialRiskSource ;
    dct:contributor _:person-harshvardhan-j-pandit ;
    dct:created "2022-08-17"^^xsd:date ;
    dct:modified "2024-08-16"^^xsd:date ;
    dct:source _:b15886bc6e88dcdb258fe59ded7be3abf ;
    vann:example dex:E0069,
        dex:E0071 ;
    rdfs:isDefinedBy risk: ;
    sw:term_status "accepted"@en ;
    skos:broader risk:SecurityBreach ;
    skos:definition "Concept representing Data Breach"@en ;
    skos:inScheme risk:risk-taxonomy-classes ;
    skos:prefLabel "Data Breach"@en .

risk:DataCollectionError a rdfs:Class,
        skos:Concept,
        dpv:RiskConcept,
        risk:PotentialConsequence,
        risk:PotentialRisk,
        risk:PotentialRiskSource ;
    dct:contributor _:person-delaram-golpayegani,
        _:person-harshvardhan-j-pandit ;
    dct:created "2024-12-01"^^xsd:date ;
    rdfs:isDefinedBy risk: ;
    sw:term_status "accepted"@en ;
    skos:broader risk:DataProcessingError ;
    skos:definition "Concept representing error related to data collection"@en ;
    skos:inScheme risk:risk-taxonomy-classes ;
    skos:prefLabel "Data Collection Error"@en .

risk:DataCorruption a rdfs:Class,
        skos:Concept,
        dpv:RiskConcept,
        risk:IntegrityConcept,
        risk:PotentialConsequence,
        risk:PotentialRisk,
        risk:PotentialRiskSource ;
    dct:contributor _:person-harshvardhan-j-pandit ;
    dct:created "2022-08-17"^^xsd:date ;
    dct:modified "2024-08-16"^^xsd:date ;
    dct:source _:b15886bc6e88dcdb258fe59ded7be3abf ;
    rdfs:isDefinedBy risk: ;
    sw:term_status "modified"@en ;
    skos:broader risk:OperationalSecurityRisk ;
    skos:definition "Concept representing Corruption of Data"@en ;
    skos:inScheme risk:risk-taxonomy-classes ;
    skos:prefLabel "Data Corruption"@en ;
    skos:scopeNote "This concept was called \"Corruption Data\" in DPV 2.0"@en .

risk:DataErasureError a rdfs:Class,
        skos:Concept,
        dpv:RiskConcept,
        risk:PotentialConsequence,
        risk:PotentialRisk,
        risk:PotentialRiskSource ;
    dct:contributor _:person-delaram-golpayegani,
        _:person-harshvardhan-j-pandit ;
    dct:created "2024-12-01"^^xsd:date ;
    rdfs:isDefinedBy risk: ;
    sw:term_status "accepted"@en ;
    skos:broader risk:DataProcessingError ;
    skos:definition "Concept representing error related to data erasure"@en ;
    skos:inScheme risk:risk-taxonomy-classes ;
    skos:prefLabel "Data Erasure Error"@en .

risk:DataInaccurate a rdfs:Class,
        skos:Concept,
        dpv:RiskConcept,
        risk:PotentialConsequence,
        risk:PotentialRisk,
        risk:PotentialRiskSource ;
    dct:contributor _:person-delaram-golpayegani,
        _:person-harshvardhan-j-pandit ;
    dct:created "2024-12-01"^^xsd:date ;
    rdfs:isDefinedBy risk: ;
    sw:term_status "accepted"@en ;
    skos:broader risk:DataRisk ;
    skos:definition "Concept representing data being inaccurate"@en ;
    skos:inScheme risk:risk-taxonomy-classes ;
    skos:prefLabel "Data Inaccurate"@en .

risk:DataIncomplete a rdfs:Class,
        skos:Concept,
        dpv:RiskConcept,
        risk:PotentialConsequence,
        risk:PotentialRisk,
        risk:PotentialRiskSource ;
    dct:contributor _:person-delaram-golpayegani,
        _:person-harshvardhan-j-pandit ;
    dct:created "2024-12-01"^^xsd:date ;
    rdfs:isDefinedBy risk: ;
    sw:term_status "accepted"@en ;
    skos:broader risk:DataRisk ;
    skos:definition "Concept representing data being incomplete"@en ;
    skos:inScheme risk:risk-taxonomy-classes ;
    skos:prefLabel "Data Incomplete"@en .

risk:DataInconsistent a rdfs:Class,
        skos:Concept,
        dpv:RiskConcept,
        risk:PotentialConsequence,
        risk:PotentialRisk,
        risk:PotentialRiskSource ;
    dct:contributor _:person-delaram-golpayegani,
        _:person-harshvardhan-j-pandit ;
    dct:created "2024-12-01"^^xsd:date ;
    rdfs:isDefinedBy risk: ;
    sw:term_status "accepted"@en ;
    skos:broader risk:DataRisk ;
    skos:definition "Concept representing data being inconsistent"@en ;
    skos:inScheme risk:risk-taxonomy-classes ;
    skos:prefLabel "Data Inconsistent"@en .

risk:DataLoss a rdfs:Class,
        skos:Concept,
        dpv:RiskConcept,
        risk:PotentialConsequence,
        risk:PotentialRisk,
        risk:PotentialRiskSource ;
    dct:contributor _:person-harshvardhan-j-pandit ;
    dct:created "2025-08-24"^^xsd:date ;
    rdfs:isDefinedBy risk: ;
    sw:term_status "accepted"@en ;
    skos:broader risk:DataRisk ;
    skos:definition "Concept representing data loss (e.g. due to errors)"@en ;
    skos:inScheme risk:risk-taxonomy-classes ;
    skos:prefLabel "Data Loss"@en .

risk:DataMisclassified a rdfs:Class,
        skos:Concept,
        dpv:RiskConcept,
        risk:PotentialConsequence,
        risk:PotentialRisk,
        risk:PotentialRiskSource ;
    dct:contributor _:person-delaram-golpayegani,
        _:person-harshvardhan-j-pandit ;
    dct:created "2024-12-01"^^xsd:date ;
    rdfs:isDefinedBy risk: ;
    sw:term_status "accepted"@en ;
    skos:broader risk:DataRisk ;
    skos:definition "Concept representing data being misclassified"@en ;
    skos:inScheme risk:risk-taxonomy-classes ;
    skos:prefLabel "Data Misclassified"@en .

risk:DataMisinterpretation a rdfs:Class,
        skos:Concept,
        dpv:RiskConcept,
        risk:PotentialConsequence,
        risk:PotentialRisk,
        risk:PotentialRiskSource ;
    dct:contributor _:person-delaram-golpayegani,
        _:person-harshvardhan-j-pandit ;
    dct:created "2024-12-01"^^xsd:date ;
    rdfs:isDefinedBy risk: ;
    sw:term_status "accepted"@en ;
    skos:broader risk:DataRisk ;
    skos:definition "Concept representing data being misinterpretation"@en ;
    skos:inScheme risk:risk-taxonomy-classes ;
    skos:prefLabel "Data Misinterpretation"@en .

risk:DataNoise a rdfs:Class,
        skos:Concept,
        dpv:RiskConcept,
        risk:PotentialConsequence,
        risk:PotentialRisk,
        risk:PotentialRiskSource ;
    dct:contributor _:person-delaram-golpayegani,
        _:person-harshvardhan-j-pandit ;
    dct:created "2024-12-01"^^xsd:date ;
    rdfs:isDefinedBy risk: ;
    sw:term_status "accepted"@en ;
    skos:broader risk:DataRisk ;
    skos:definition "Concept representing data being noise"@en ;
    skos:inScheme risk:risk-taxonomy-classes ;
    skos:prefLabel "Data Noise"@en .

risk:DataOutdated a rdfs:Class,
        skos:Concept,
        dpv:RiskConcept,
        risk:PotentialConsequence,
        risk:PotentialRisk,
        risk:PotentialRiskSource ;
    dct:contributor _:person-delaram-golpayegani,
        _:person-harshvardhan-j-pandit ;
    dct:created "2024-12-01"^^xsd:date ;
    rdfs:isDefinedBy risk: ;
    sw:term_status "accepted"@en ;
    skos:broader risk:DataRisk ;
    skos:definition "Concept representing data being outdated"@en ;
    skos:inScheme risk:risk-taxonomy-classes ;
    skos:prefLabel "Data Outdated"@en .

risk:DataPreparationError a rdfs:Class,
        skos:Concept,
        dpv:RiskConcept,
        risk:PotentialConsequence,
        risk:PotentialRisk,
        risk:PotentialRiskSource ;
    dct:contributor _:person-delaram-golpayegani,
        _:person-harshvardhan-j-pandit ;
    dct:created "2024-12-01"^^xsd:date ;
    rdfs:isDefinedBy risk: ;
    sw:term_status "accepted"@en ;
    skos:broader risk:DataProcessingError ;
    skos:definition "Concept representing error related to data preparation"@en ;
    skos:inScheme risk:risk-taxonomy-classes ;
    skos:prefLabel "Data Preparation Error"@en .

risk:DataProcessingBias a rdfs:Class,
        skos:Concept,
        dpv:RiskConcept,
        risk:PotentialConsequence,
        risk:PotentialRisk,
        risk:PotentialRiskSource ;
    dct:contributor _:person-daniel-doherty,
        _:person-delaram-golpayegani,
        _:person-harshvardhan-j-pandit ;
    dct:created "2024-09-13"^^xsd:date ;
    dct:source "ISO/IEC 24027:2021"@en ;
    rdfs:isDefinedBy risk: ;
    sw:term_status "accepted"@en ;
    skos:broader risk:DataBias ;
    skos:definition "Bias that occurs due to pre-processing (or post-processing) of data, even though the original data would not have led to any bias"@en ;
    skos:inScheme risk:risk-taxonomy-classes ;
    skos:prefLabel "Data Processing Bias"@en .

risk:DataProcessingError a rdfs:Class,
        skos:Concept,
        dpv:RiskConcept,
        risk:PotentialConsequence,
        risk:PotentialRisk,
        risk:PotentialRiskSource ;
    dct:contributor _:person-delaram-golpayegani,
        _:person-harshvardhan-j-pandit ;
    dct:created "2024-12-01"^^xsd:date ;
    rdfs:isDefinedBy risk: ;
    sw:term_status "accepted"@en ;
    skos:broader risk:DataRisk ;
    skos:definition "Concept representing operational error in the processing of data"@en ;
    skos:inScheme risk:risk-taxonomy-classes ;
    skos:prefLabel "Data Processing Error"@en .

risk:DataRisk a rdfs:Class,
        skos:Concept,
        dpv:RiskConcept,
        risk:PotentialConsequence,
        risk:PotentialRisk,
        risk:PotentialRiskSource ;
    dct:contributor _:person-delaram-golpayegani,
        _:person-harshvardhan-j-pandit ;
    dct:created "2024-12-01"^^xsd:date ;
    rdfs:isDefinedBy risk: ;
    sw:term_status "accepted"@en ;
    skos:broader risk:TechnicalRiskConcept ;
    skos:definition "Risks and risk concepts related to data"@en ;
    skos:inScheme risk:risk-taxonomy-classes ;
    skos:prefLabel "Data Risk"@en .

risk:DataSelectionError a rdfs:Class,
        skos:Concept,
        dpv:RiskConcept,
        risk:PotentialConsequence,
        risk:PotentialRisk,
        risk:PotentialRiskSource ;
    dct:contributor _:person-delaram-golpayegani,
        _:person-harshvardhan-j-pandit ;
    dct:created "2024-12-01"^^xsd:date ;
    rdfs:isDefinedBy risk: ;
    sw:term_status "accepted"@en ;
    skos:broader risk:DataProcessingError ;
    skos:definition "Concept representing an error in data selection"@en ;
    skos:inScheme risk:risk-taxonomy-classes ;
    skos:prefLabel "Data SelectionError"@en .

risk:DataSparse a rdfs:Class,
        skos:Concept,
        dpv:RiskConcept,
        risk:PotentialConsequence,
        risk:PotentialRisk,
        risk:PotentialRiskSource ;
    dct:contributor _:person-delaram-golpayegani,
        _:person-harshvardhan-j-pandit ;
    dct:created "2024-12-01"^^xsd:date ;
    rdfs:isDefinedBy risk: ;
    sw:term_status "accepted"@en ;
    skos:broader risk:DataRisk ;
    skos:definition "Concept representing data being sparse"@en ;
    skos:inScheme risk:risk-taxonomy-classes ;
    skos:prefLabel "Data Sparse"@en .

risk:DataStorageError a rdfs:Class,
        skos:Concept,
        dpv:RiskConcept,
        risk:PotentialConsequence,
        risk:PotentialRisk,
        risk:PotentialRiskSource ;
    dct:contributor _:person-delaram-golpayegani,
        _:person-harshvardhan-j-pandit ;
    dct:created "2024-12-01"^^xsd:date ;
    rdfs:isDefinedBy risk: ;
    sw:term_status "accepted"@en ;
    skos:broader risk:DataProcessingError ;
    skos:definition "Concept representing error related to data storage"@en ;
    skos:inScheme risk:risk-taxonomy-classes ;
    skos:prefLabel "Data Storage Error"@en .

risk:DataTransferError a rdfs:Class,
        skos:Concept,
        dpv:RiskConcept,
        risk:PotentialConsequence,
        risk:PotentialRisk,
        risk:PotentialRiskSource ;
    dct:contributor _:person-delaram-golpayegani,
        _:person-harshvardhan-j-pandit ;
    dct:created "2024-12-01"^^xsd:date ;
    rdfs:isDefinedBy risk: ;
    sw:term_status "accepted"@en ;
    skos:broader risk:DataProcessingError ;
    skos:definition "Concept representing error related to data transfer"@en ;
    skos:inScheme risk:risk-taxonomy-classes ;
    skos:prefLabel "Data Transfer Error"@en .

risk:DataUnavailable a rdfs:Class,
        skos:Concept,
        dpv:RiskConcept,
        risk:PotentialConsequence,
        risk:PotentialRisk,
        risk:PotentialRiskSource ;
    dct:contributor _:person-delaram-golpayegani,
        _:person-harshvardhan-j-pandit ;
    dct:created "2024-12-01"^^xsd:date ;
    rdfs:isDefinedBy risk: ;
    sw:term_status "accepted"@en ;
    skos:broader risk:DataRisk ;
    skos:definition "Concept representing data being unavailable"@en ;
    skos:inScheme risk:risk-taxonomy-classes ;
    skos:prefLabel "Data Unavailable"@en .

risk:DataUnrepresentative a rdfs:Class,
        skos:Concept,
        dpv:RiskConcept,
        risk:PotentialConsequence,
        risk:PotentialRisk,
        risk:PotentialRiskSource ;
    dct:contributor _:person-delaram-golpayegani,
        _:person-harshvardhan-j-pandit ;
    dct:created "2024-12-01"^^xsd:date ;
    rdfs:isDefinedBy risk: ;
    sw:term_status "accepted"@en ;
    skos:broader risk:DataRisk ;
    skos:definition "Concept representing data being unrepresentative"@en ;
    skos:inScheme risk:risk-taxonomy-classes ;
    skos:prefLabel "Data Unrepresentative"@en .

risk:DataUnstructured a rdfs:Class,
        skos:Concept,
        dpv:RiskConcept,
        risk:PotentialConsequence,
        risk:PotentialRisk,
        risk:PotentialRiskSource ;
    dct:contributor _:person-delaram-golpayegani,
        _:person-harshvardhan-j-pandit ;
    dct:created "2024-12-01"^^xsd:date ;
    rdfs:isDefinedBy risk: ;
    sw:term_status "accepted"@en ;
    skos:broader risk:DataRisk ;
    skos:definition "Concept representing data being unstructured"@en ;
    skos:inScheme risk:risk-taxonomy-classes ;
    skos:prefLabel "Data Unstructured"@en .

risk:DataUnverified a rdfs:Class,
        skos:Concept,
        dpv:RiskConcept,
        risk:PotentialConsequence,
        risk:PotentialRisk,
        risk:PotentialRiskSource ;
    dct:contributor _:person-delaram-golpayegani,
        _:person-harshvardhan-j-pandit ;
    dct:created "2024-12-01"^^xsd:date ;
    rdfs:isDefinedBy risk: ;
    sw:term_status "accepted"@en ;
    skos:broader risk:DataRisk ;
    skos:definition "Concept representing data being unverified"@en ;
    skos:inScheme risk:risk-taxonomy-classes ;
    skos:prefLabel "Data Unverified"@en .

risk:Deception a rdfs:Class,
        skos:Concept,
        dpv:RiskConcept,
        risk:ConfidentialityConcept,
        risk:IntegrityConcept,
        risk:PotentialConsequence,
        risk:PotentialRisk,
        risk:PotentialRiskSource ;
    dct:contributor _:person-delaram-golpayegani ;
    dct:created "2026-02-09"^^xsd:date ;
    rdfs:isDefinedBy risk: ;
    sw:term_status "accepted"@en ;
    skos:broader risk:MaliciousActivity ;
    skos:definition "Concept representing Deception"@en ;
    skos:inScheme risk:risk-taxonomy-classes ;
    skos:prefLabel "Deception"@en .

risk:DelayedApplicationProcessing a rdfs:Class,
        skos:Concept,
        dpv:RiskConcept,
        risk:PotentialConsequence,
        risk:PotentialImpact,
        risk:PotentialRisk ;
    dct:created "2024-10-21"^^xsd:date ;
    rdfs:isDefinedBy risk: ;
    sw:term_status "accepted"@en ;
    skos:broader risk:ServiceRelatedConsequence ;
    skos:definition "Concept representing delayed processing of applications"@en ;
    skos:inScheme risk:risk-taxonomy-classes ;
    skos:prefLabel "Delayed Application Processing"@en .

risk:DeliberateIncident a rdfs:Class,
        skos:Concept ;
    dct:created "2024-05-19"^^xsd:date ;
    rdfs:isDefinedBy risk: ;
    rdfs:subClassOf risk:Incident ;
    sw:term_status "accepted"@en ;
    skos:broader risk:Incident ;
    skos:definition "Incident caused due to deliberate actions of a human"@en ;
    skos:inScheme risk:incident-classes ;
    skos:prefLabel "Deliberate Incident"@en .

risk:DenialServiceAttack a rdfs:Class,
        skos:Concept,
        dpv:RiskConcept,
        risk:AvailabilityConcept,
        risk:PotentialRisk,
        risk:PotentialRiskSource ;
    dct:contributor _:person-harshvardhan-j-pandit ;
    dct:created "2022-08-17"^^xsd:date ;
    dct:modified "2024-08-16"^^xsd:date ;
    dct:source _:b15886bc6e88dcdb258fe59ded7be3abf ;
    rdfs:isDefinedBy risk: ;
    sw:term_status "accepted"@en ;
    skos:broader risk:SecurityAttack ;
    skos:definition "Concept representing Denial of Service Attack (DoS)"@en ;
    skos:inScheme risk:risk-taxonomy-classes ;
    skos:prefLabel "Denial of Service Attack (DoS)"@en .

risk:DetectionControl a rdfs:Class,
        skos:Concept,
        risk:RiskControl ;
    dct:contributor _:person-delaram-golpayegani,
        _:person-harshvardhan-j-pandit ;
    dct:created "2024-05-19"^^xsd:date ;
    dct:modified "2025-01-06"^^xsd:date ;
    rdfs:isDefinedBy risk: ;
    sw:term_status "modified"@en ;
    skos:broader risk:MonitorControl ;
    skos:definition "Control that detects an event"@en ;
    skos:inScheme risk:risk-controls-classes ;
    skos:prefLabel "Detection Control"@en ;
    skos:scopeNote "Detection refers to the observation, derivation, inference, or any other method for drawing conclusions that an event has occurred or is likely to occur with a given certainty. For controls that identify information about the event in terms of metrics or characteristics, see risk:IdentificationControl"@en .

risk:Detriment a rdfs:Class,
        skos:Concept,
        dpv:RiskConcept,
        risk:PotentialConsequence,
        risk:PotentialImpact,
        risk:PotentialRisk ;
    dct:contributor _:person-beatriz-esteves,
        _:person-fajar-ekaputra,
        _:person-georg-p-krog,
        _:person-harshvardhan-j-pandit,
        _:person-julian-flake ;
    dct:created "2022-03-23"^^xsd:date ;
    dct:modified "2024-08-16"^^xsd:date ;
    rdfs:isDefinedBy risk: ;
    sw:term_status "accepted"@en ;
    skos:broader risk:LegallyRelevantConsequence ;
    skos:definition "Concept representing Detriment"@en ;
    skos:inScheme risk:risk-taxonomy-classes ;
    skos:prefLabel "Detriment"@en .

risk:DirectDiscrimination a rdfs:Class,
        skos:Concept,
        dpv:RiskConcept,
        risk:PotentialConsequence,
        risk:PotentialImpact,
        risk:PotentialRisk ;
    dct:created "2024-09-30"^^xsd:date ;
    rdfs:isDefinedBy risk: ;
    sw:term_status "accepted"@en ;
    skos:broader risk:Discrimination ;
    skos:definition "Occurs when a person is treated less favourably than another in a comparable situation based on a protected characteristic (e.g., race, sex, disability)"@en ;
    skos:inScheme risk:risk-taxonomy-classes ;
    skos:prefLabel "Direct Discrimination"@en .

risk:DisabilityDiscrimination a rdfs:Class,
        skos:Concept,
        dpv:RiskConcept,
        risk:PotentialConsequence,
        risk:PotentialImpact,
        risk:PotentialRisk ;
    dct:created "2024-09-30"^^xsd:date ;
    rdfs:isDefinedBy risk: ;
    sw:term_status "accepted"@en ;
    skos:broader risk:Discrimination ;
    skos:definition "Discrimination against individuals based on physical or mental disabilities"@en ;
    skos:inScheme risk:risk-taxonomy-classes ;
    skos:prefLabel "Disability Discrimination"@en .

risk:Discrimination a rdfs:Class,
        skos:Concept,
        dpv:RiskConcept,
        risk:PotentialConsequence,
        risk:PotentialImpact,
        risk:PotentialRisk ;
    dct:contributor _:person-georg-p-krog ;
    dct:created "2024-09-30"^^xsd:date ;
    rdfs:isDefinedBy risk: ;
    sw:term_status "accepted"@en ;
    skos:broader risk:SocietalRiskConcept ;
    skos:definition "Discrimination is the treatment of a person or particular group of people differently, in a way that is worse than the way people are usually treated"@en ;
    skos:inScheme risk:risk-taxonomy-classes ;
    skos:prefLabel "Discrimination"@en .

risk:DisproportionateEnergyConsumption a rdfs:Class,
        skos:Concept,
        dpv:RiskConcept,
        risk:PotentialConsequence,
        risk:PotentialImpact,
        risk:PotentialRisk ;
    dct:created "2024-10-21"^^xsd:date ;
    rdfs:isDefinedBy risk: ;
    sw:term_status "accepted"@en ;
    skos:broader risk:EnvironmentalRisk ;
    skos:definition "The occurrence or potential occurrence of disproportionate energy consumption when considering the value obtained from undertaking the activity and the amount of energy being utilised"@en ;
    skos:inScheme risk:risk-taxonomy-classes ;
    skos:prefLabel "Disproportionate Energy Consumption"@en .

risk:DistributedDenialServiceAttack a rdfs:Class,
        skos:Concept,
        dpv:RiskConcept,
        risk:AvailabilityConcept,
        risk:PotentialRisk,
        risk:PotentialRiskSource ;
    dct:contributor _:person-harshvardhan-j-pandit ;
    dct:created "2022-08-17"^^xsd:date ;
    dct:modified "2024-08-16"^^xsd:date ;
    dct:source _:b15886bc6e88dcdb258fe59ded7be3abf ;
    rdfs:isDefinedBy risk: ;
    sw:term_status "accepted"@en ;
    skos:broader risk:DenialServiceAttack ;
    skos:definition "Concept representing Distributed Denial of Service Attack (DDoS)"@en ;
    skos:inScheme risk:risk-taxonomy-classes ;
    skos:prefLabel "Distributed Denial of Service Attack (DDoS)"@en .

risk:DocumentationIssues a rdfs:Class,
        skos:Concept,
        dpv:RiskConcept,
        risk:PotentialConsequence,
        risk:PotentialRisk,
        risk:PotentialRiskSource ;
    dct:contributor _:person-delaram-golpayegani ;
    dct:created "2026-02-09"^^xsd:date ;
    rdfs:isDefinedBy risk: ;
    sw:term_status "accepted"@en ;
    skos:broader risk:OrganisationalManagementRisk ;
    skos:definition "Concept representing issues with the development and use of documentation"@en ;
    skos:inScheme risk:risk-taxonomy-classes ;
    skos:prefLabel "Documentation Issues"@en .

risk:Earthquake a rdfs:Class,
        skos:Concept,
        dpv:RiskConcept,
        risk:PotentialConsequence,
        risk:PotentialImpact,
        risk:PotentialRisk ;
    dct:created "2024-10-21"^^xsd:date ;
    rdfs:isDefinedBy risk: ;
    sw:term_status "accepted"@en ;
    skos:broader risk:EnvironmentalRisk ;
    skos:definition "The occurrence or potential occurrence of earthquakes"@en ;
    skos:inScheme risk:risk-taxonomy-classes ;
    skos:prefLabel "Earthquake"@en .

risk:EliminationControl a rdfs:Class,
        skos:Concept,
        risk:RiskControl ;
    dct:contributor _:person-delaram-golpayegani,
        _:person-harshvardhan-j-pandit ;
    dct:created "2025-01-06"^^xsd:date ;
    rdfs:isDefinedBy risk: ;
    sw:term_status "accepted"@en ;
    skos:broader risk:AvoidanceControl ;
    skos:definition "Control that eliminates an event entirely such that the event does not occur"@en ;
    skos:inScheme risk:risk-controls-classes ;
    skos:prefLabel "Elimination Control"@en ;
    skos:scopeNote "Elimination requires the event's likelihood to be reduced to zero such that the event cannot occur in the context. This can be done by establishing methods to prevent the event from occurring (e.g. gatekeeping filters) or by changing the underlying context (e.g. replacing faulty device). The difference between risk:ModificationControl and risk:EliminationControl is that modification works to change the event characteristics whereas elimination works on the context to prevent the event"@en .

risk:EnvironmentalIncident a rdfs:Class,
        skos:Concept ;
    dct:created "2024-05-19"^^xsd:date ;
    rdfs:isDefinedBy risk: ;
    rdfs:subClassOf risk:Incident ;
    sw:term_status "accepted"@en ;
    skos:broader risk:Incident ;
    skos:definition "Incident caused due to environmental factors outside human controls"@en ;
    skos:inScheme risk:incident-classes ;
    skos:prefLabel "Environmental Incident"@en .

risk:EnvironmentalRisk a rdfs:Class,
        skos:Concept,
        dpv:RiskConcept,
        risk:PotentialConsequence,
        risk:PotentialImpact,
        risk:PotentialRisk ;
    dct:created "2024-10-21"^^xsd:date ;
    rdfs:isDefinedBy risk: ;
    sw:term_status "accepted"@en ;
    skos:broader risk:SocietalRiskConcept ;
    skos:definition "Risks and issues that have their origin in environment or can affect the environment at large"@en ;
    skos:inScheme risk:risk-taxonomy-classes ;
    skos:prefLabel "Environmental Risk"@en .

risk:EquipmentFailure a rdfs:Class,
        skos:Concept,
        dpv:RiskConcept,
        risk:AvailabilityConcept,
        risk:PotentialConsequence,
        risk:PotentialRisk,
        risk:PotentialRiskSource ;
    dct:contributor _:person-harshvardhan-j-pandit ;
    dct:created "2022-08-17"^^xsd:date ;
    dct:modified "2024-08-16"^^xsd:date ;
    dct:source _:b15886bc6e88dcdb258fe59ded7be3abf ;
    rdfs:isDefinedBy risk: ;
    sw:term_status "accepted"@en ;
    skos:broader risk:OperationalSecurityRisk ;
    skos:definition "Concept representing Equipment Failure"@en ;
    skos:inScheme risk:risk-taxonomy-classes ;
    skos:prefLabel "Equipment Failure"@en ;
    skos:scopeNote "Here equipment refers to physical equipment"@en .

risk:EquipmentMalfunction a rdfs:Class,
        skos:Concept,
        dpv:RiskConcept,
        risk:AvailabilityConcept,
        risk:PotentialConsequence,
        risk:PotentialRisk,
        risk:PotentialRiskSource ;
    dct:contributor _:person-harshvardhan-j-pandit ;
    dct:created "2022-08-17"^^xsd:date ;
    dct:modified "2024-08-16"^^xsd:date ;
    dct:source _:b15886bc6e88dcdb258fe59ded7be3abf ;
    rdfs:isDefinedBy risk: ;
    sw:term_status "accepted"@en ;
    skos:broader risk:OperationalSecurityRisk ;
    skos:definition "Concept representing Equipment Malfunction"@en ;
    skos:inScheme risk:risk-taxonomy-classes ;
    skos:prefLabel "Equipment Malfunction"@en ;
    skos:scopeNote "Here equipment refers to physical equipment"@en .

risk:ErroneousUse a rdfs:Class,
        skos:Concept,
        dpv:RiskConcept,
        risk:PotentialConsequence,
        risk:PotentialRisk,
        risk:PotentialRiskSource ;
    dct:contributor _:person-harshvardhan-j-pandit ;
    dct:created "2022-08-17"^^xsd:date ;
    dct:modified "2024-08-16"^^xsd:date ;
    dct:source _:b15886bc6e88dcdb258fe59ded7be3abf ;
    rdfs:isDefinedBy risk: ;
    sw:term_status "accepted"@en ;
    skos:broader risk:UserRisks ;
    skos:definition "Concept representing erroneous use (of something)"@en ;
    skos:inScheme risk:risk-taxonomy-classes ;
    skos:prefLabel "Erroneous Use"@en .

risk:EthnicDiscrimination a rdfs:Class,
        skos:Concept,
        dpv:RiskConcept,
        risk:PotentialConsequence,
        risk:PotentialImpact,
        risk:PotentialRisk ;
    dct:created "2024-09-30"^^xsd:date ;
    rdfs:isDefinedBy risk: ;
    sw:term_status "accepted"@en ;
    skos:broader risk:Racism ;
    skos:definition "Discrimination against individuals based on their ethnicity or cultural heritage"@en ;
    skos:inScheme risk:risk-taxonomy-classes ;
    skos:prefLabel "Ethnic Discrimination"@en .

risk:ExcellenceDiscrimination a rdfs:Class,
        skos:Concept,
        dpv:RiskConcept,
        risk:PotentialConsequence,
        risk:PotentialImpact,
        risk:PotentialRisk ;
    dct:created "2024-09-30"^^xsd:date ;
    rdfs:isDefinedBy risk: ;
    sw:term_status "accepted"@en ;
    skos:broader risk:Discrimination ;
    skos:definition "Favouritism towards individuals deemed more competent or superior, often at the expense of others"@en ;
    skos:inScheme risk:risk-taxonomy-classes ;
    skos:prefLabel "Excellence Discrimination"@en .

risk:Exploitation a rdfs:Class,
        skos:Concept,
        dpv:RiskConcept,
        risk:ConfidentialityConcept,
        risk:IntegrityConcept,
        risk:PotentialConsequence,
        risk:PotentialRisk,
        risk:PotentialRiskSource ;
    dct:contributor _:person-delaram-golpayegani ;
    dct:created "2026-02-09"^^xsd:date ;
    rdfs:isDefinedBy risk: ;
    sw:term_status "accepted"@en ;
    skos:broader risk:MaliciousActivity ;
    skos:definition "Concept representing Exploitation"@en ;
    skos:inScheme risk:risk-taxonomy-classes ;
    skos:prefLabel "Exploitation"@en .

risk:ExposureToHarmfulSpeech a rdfs:Class,
        skos:Concept,
        dpv:RiskConcept,
        risk:PotentialConsequence,
        risk:PotentialImpact,
        risk:PotentialRisk ;
    dct:contributor _:person-harshvardhan-j-pandit ;
    dct:created "2022-08-17"^^xsd:date ;
    dct:modified "2024-08-16"^^xsd:date ;
    dct:source _:b7191aa21b975cb14bbce32aa3ba9c7eb ;
    rdfs:isDefinedBy risk: ;
    sw:term_status "accepted"@en ;
    skos:broader risk:IndividualRisk,
        risk:MentalHealth,
        risk:Wellbeing ;
    skos:definition "Concept representing Harmful Speech"@en ;
    skos:inScheme risk:risk-taxonomy-classes ;
    skos:prefLabel "Exposure to Harmful Speech"@en ;
    skos:scopeNote "This concept was called \"HarmfulSpeech\" in DPV 2.0"@en .

risk:ExternalSecurityThreat a rdfs:Class,
        skos:Concept,
        dpv:RiskConcept,
        risk:PotentialConsequence,
        risk:PotentialRisk,
        risk:PotentialRiskSource ;
    dct:created "2024-12-17"^^xsd:date ;
    rdfs:isDefinedBy risk: ;
    sw:term_status "accepted"@en ;
    skos:broader risk:TechnicalRiskConcept ;
    skos:definition "Concepts associated with security threats that are likely to originate externally"@en ;
    skos:inScheme risk:risk-taxonomy-classes ;
    skos:prefLabel "External Security Threat"@en .

risk:Extortion a rdfs:Class,
        skos:Concept,
        dpv:RiskConcept,
        risk:ConfidentialityConcept,
        risk:PotentialConsequence,
        risk:PotentialRisk,
        risk:PotentialRiskSource ;
    dct:contributor _:person-arthit-suriyawongkul,
        _:person-harshvardhan-j-pandit ;
    dct:created "2022-08-17"^^xsd:date ;
    dct:modified "2025-08-06"^^xsd:date ;
    dct:source _:b65de0d403668931587d7f38d790f5adc ;
    rdfs:isDefinedBy risk: ;
    sw:term_status "modified"@en ;
    skos:broader risk:Exploitation ;
    skos:definition "Concept representing Extortion"@en ;
    skos:inScheme risk:risk-taxonomy-classes ;
    skos:prefLabel "Extortion"@en .

risk:ExtremelyHighLikelihood a rdfs:Class,
        skos:Concept,
        dpv:Likelihood ;
    dct:contributor _:person-harshvardhan-j-pandit ;
    dct:created "2022-08-18"^^xsd:date ;
    rdf:value 0.99 ;
    rdfs:isDefinedBy risk: ;
    sw:term_status "accepted"@en ;
    skos:broader risk:7LikelihoodLevels ;
    skos:definition "Level where Likelihood is Extremely High"@en ;
    skos:inScheme risk:risk-levels-classes ;
    skos:prefLabel "Extremely High Likelihood"@en ;
    skos:scopeNote "The suggested quantitative value for this concept is 0.99 on a scale of 0 to 1"@en .

risk:ExtremelyHighRisk a rdfs:Class,
        skos:Concept,
        dpv:RiskLevel ;
    dct:contributor _:person-harshvardhan-j-pandit ;
    dct:created "2022-08-18"^^xsd:date ;
    rdf:value 0.99 ;
    rdfs:isDefinedBy risk: ;
    sw:term_status "accepted"@en ;
    skos:broader risk:7RiskLevels ;
    skos:definition "Level where Risk is Extremely High"@en ;
    skos:inScheme risk:risk-levels-classes ;
    skos:prefLabel "Extremely High Risk"@en ;
    skos:scopeNote "The suggested quantitative value for this concept is 0.99 on a scale of 0 to 1"@en .

risk:ExtremelyHighSeverity a rdfs:Class,
        skos:Concept,
        dpv:Severity ;
    dct:contributor _:person-harshvardhan-j-pandit ;
    dct:created "2022-08-18"^^xsd:date ;
    rdf:value 0.99 ;
    rdfs:isDefinedBy risk: ;
    sw:term_status "accepted"@en ;
    skos:broader risk:7SeverityLevels ;
    skos:definition "Level where Severity is Extremely High"@en ;
    skos:inScheme risk:risk-levels-classes ;
    skos:prefLabel "Extremely High Severity"@en ;
    skos:scopeNote "The suggested quantitative value for this concept is 0.99 on a scale of 0 to 1"@en .

risk:ExtremelyLowLikelihood a rdfs:Class,
        skos:Concept,
        dpv:Likelihood ;
    dct:contributor _:person-harshvardhan-j-pandit ;
    dct:created "2022-08-18"^^xsd:date ;
    rdf:value 0.01 ;
    rdfs:isDefinedBy risk: ;
    sw:term_status "accepted"@en ;
    skos:broader risk:7LikelihoodLevels ;
    skos:definition "Level where Likelihood is Extremely Low"@en ;
    skos:inScheme risk:risk-levels-classes ;
    skos:prefLabel "Extremely Low Likelihood"@en ;
    skos:scopeNote "The suggested quantitative value for this concept is 0.01 on a scale of 0 to 1"@en .

risk:ExtremelyLowRisk a rdfs:Class,
        skos:Concept,
        dpv:RiskLevel ;
    dct:contributor _:person-harshvardhan-j-pandit ;
    dct:created "2022-08-18"^^xsd:date ;
    rdf:value 0.01 ;
    rdfs:isDefinedBy risk: ;
    sw:term_status "accepted"@en ;
    skos:broader risk:7RiskLevels ;
    skos:definition "Level where Risk is Extremely Low"@en ;
    skos:inScheme risk:risk-levels-classes ;
    skos:prefLabel "Extremely Low Risk"@en ;
    skos:scopeNote "The suggested quantitative value for this concept is 0.01 on a scale of 0 to 1"@en .

risk:ExtremelyLowSeverity a rdfs:Class,
        skos:Concept,
        dpv:Severity ;
    dct:contributor _:person-harshvardhan-j-pandit ;
    dct:created "2022-08-18"^^xsd:date ;
    rdf:value 0.01 ;
    rdfs:isDefinedBy risk: ;
    sw:term_status "accepted"@en ;
    skos:broader risk:7SeverityLevels ;
    skos:definition "Level where Severity is Extremely Low"@en ;
    skos:inScheme risk:risk-levels-classes ;
    skos:prefLabel "Extremely Low Severity"@en ;
    skos:scopeNote "The suggested quantitative value for this concept is 0.01 on a scale of 0 to 1"@en .

risk:FinancialImpact a rdfs:Class,
        skos:Concept,
        dpv:RiskConcept,
        risk:PotentialConsequence,
        risk:PotentialImpact,
        risk:PotentialRisk ;
    dct:created "2024-10-21"^^xsd:date ;
    rdfs:isDefinedBy risk: ;
    sw:term_status "accepted"@en ;
    skos:broader risk:OrganisationalRiskConcept ;
    skos:definition "Things that cause or have the potential to impact financial resources"@en ;
    skos:inScheme risk:risk-taxonomy-classes ;
    skos:prefLabel "Financial Impact"@en .

risk:FinancialLoss a rdfs:Class,
        skos:Concept,
        dpv:RiskConcept,
        risk:PotentialConsequence,
        risk:PotentialImpact,
        risk:PotentialRisk ;
    dct:contributor _:person-harshvardhan-j-pandit ;
    dct:created "2022-08-17"^^xsd:date ;
    dct:modified "2024-08-16"^^xsd:date ;
    dct:source _:b15886bc6e88dcdb258fe59ded7be3abf ;
    rdfs:isDefinedBy risk: ;
    sw:term_status "accepted"@en ;
    skos:broader risk:FinancialImpact ;
    skos:definition "Concept representing Financial Loss which may be actual loss of existing financial assets or hypothetical loss of financial opportunity"@en ;
    skos:inScheme risk:risk-taxonomy-classes ;
    skos:prefLabel "Financial Loss"@en .

risk:Floods a rdfs:Class,
        skos:Concept,
        dpv:RiskConcept,
        risk:PotentialConsequence,
        risk:PotentialImpact,
        risk:PotentialRisk ;
    dct:created "2024-10-21"^^xsd:date ;
    rdfs:isDefinedBy risk: ;
    sw:term_status "accepted"@en ;
    skos:broader risk:EnvironmentalRisk ;
    skos:definition "The occurrence or potential occurrence of floods"@en ;
    skos:inScheme risk:risk-taxonomy-classes ;
    skos:prefLabel "Floods"@en .

risk:Fraud a rdfs:Class,
        skos:Concept,
        dpv:RiskConcept,
        risk:ConfidentialityConcept,
        risk:PotentialConsequence,
        risk:PotentialRisk,
        risk:PotentialRiskSource ;
    dct:contributor _:person-harshvardhan-j-pandit ;
    dct:created "2022-08-17"^^xsd:date ;
    dct:modified "2026-02-09"^^xsd:date ;
    dct:source _:b15886bc6e88dcdb258fe59ded7be3abf ;
    rdfs:isDefinedBy risk: ;
    sw:term_status "modified"@en ;
    skos:broader risk:Deception ;
    skos:definition "Concept representing Fraud"@en ;
    skos:inScheme risk:risk-taxonomy-classes ;
    skos:prefLabel "Fraud"@en .

risk:GenderDiscrimination a rdfs:Class,
        skos:Concept,
        dpv:RiskConcept,
        risk:PotentialConsequence,
        risk:PotentialImpact,
        risk:PotentialRisk ;
    dct:created "2024-09-30"^^xsd:date ;
    rdfs:isDefinedBy risk: ;
    sw:term_status "accepted"@en ;
    skos:broader risk:Sexism ;
    skos:definition "Discrimination based on a person's gender identity or gender expression"@en ;
    skos:inScheme risk:risk-taxonomy-classes ;
    skos:prefLabel "Gender Discrimination"@en .

risk:GeographicDiscrimination a rdfs:Class,
        skos:Concept,
        dpv:RiskConcept,
        risk:PotentialConsequence,
        risk:PotentialImpact,
        risk:PotentialRisk ;
    dct:created "2024-09-30"^^xsd:date ;
    rdfs:isDefinedBy risk: ;
    sw:term_status "accepted"@en ;
    skos:broader risk:Discrimination ;
    skos:definition "Discrimination based on a person's geographical origin or residence"@en ;
    skos:inScheme risk:risk-taxonomy-classes ;
    skos:prefLabel "Geographic Discrimination"@en .

risk:GoodwillLoss a rdfs:Class,
        skos:Concept,
        dpv:RiskConcept,
        risk:PotentialConsequence,
        risk:PotentialImpact,
        risk:PotentialRisk ;
    dct:contributor _:person-harshvardhan-j-pandit ;
    dct:created "2022-08-17"^^xsd:date ;
    dct:modified "2025-08-24"^^xsd:date ;
    dct:source _:b15886bc6e88dcdb258fe59ded7be3abf ;
    rdfs:isDefinedBy risk: ;
    sw:term_status "modified"@en ;
    skos:broader risk:ReputationalRisk ;
    skos:definition "Concept representing Goodwill Loss"@en ;
    skos:inScheme risk:risk-taxonomy-classes ;
    skos:prefLabel "Goodwill Loss"@en .

risk:GroupAttributionBias a rdfs:Class,
        skos:Concept,
        dpv:RiskConcept,
        risk:PotentialConsequence,
        risk:PotentialRisk,
        risk:PotentialRiskSource ;
    dct:contributor _:person-daniel-doherty,
        _:person-delaram-golpayegani,
        _:person-harshvardhan-j-pandit ;
    dct:created "2024-09-13"^^xsd:date ;
    dct:source "ISO/IEC 24027:2021"@en ;
    rdfs:isDefinedBy risk: ;
    sw:term_status "accepted"@en ;
    skos:broader risk:CognitiveBias ;
    skos:definition "Bias that occurs when a human assumes that what is true for an individual or object is also true for everyone, or all objects, in that group"@en ;
    skos:inScheme risk:risk-taxonomy-classes ;
    skos:prefLabel "Group Attribution Bias"@en .

risk:GroupHealthSafety a rdfs:Class,
        skos:Concept,
        dpv:RiskConcept,
        risk:PotentialConsequence,
        risk:PotentialImpact,
        risk:PotentialRisk ;
    dct:created "2024-12-01"^^xsd:date ;
    rdfs:isDefinedBy risk: ;
    sw:term_status "accepted"@en ;
    skos:broader risk:GroupRisk,
        risk:HealthSafety ;
    skos:definition "Concept representing health & safety of a group or group(s)"@en ;
    skos:inScheme risk:risk-taxonomy-classes ;
    skos:prefLabel "Group Health & Safety"@en .

risk:GroupRisk a rdfs:Class,
        skos:Concept,
        dpv:RiskConcept,
        risk:PotentialConsequence,
        risk:PotentialImpact,
        risk:PotentialRisk ;
    dct:created "2024-12-17"^^xsd:date ;
    rdfs:isDefinedBy risk: ;
    sw:term_status "accepted"@en ;
    skos:broader risk:SocietalRiskConcept ;
    skos:definition "Risks and issues that affect or have the potential to affect groups in society"@en ;
    skos:inScheme risk:risk-taxonomy-classes ;
    skos:prefLabel "Societal Risk"@en .

risk:HaltConsequence a rdfs:Class,
        skos:Concept,
        risk:RiskControl ;
    dct:contributor _:person-harshvardhan-j-pandit ;
    dct:created "2025-01-06"^^xsd:date ;
    rdfs:isDefinedBy risk: ;
    sw:term_status "accepted"@en ;
    skos:broader risk:ConsequenceControl,
        risk:InterruptionControl ;
    skos:definition "Control that halts the (ongoing) consequence event or process such that it no longer takes place or is applicable in the context"@en ;
    skos:inScheme risk:risk-controls-classes ;
    skos:prefLabel "Halt Consequence"@en .

risk:HaltImpact a rdfs:Class,
        skos:Concept,
        risk:RiskControl ;
    dct:contributor _:person-harshvardhan-j-pandit ;
    dct:created "2025-01-06"^^xsd:date ;
    rdfs:isDefinedBy risk: ;
    sw:term_status "accepted"@en ;
    skos:broader risk:ImpactControl,
        risk:InterruptionControl ;
    skos:definition "Control that halts the (ongoing) impact event or process such that it no longer takes place or is applicable in the context"@en ;
    skos:inScheme risk:risk-controls-classes ;
    skos:prefLabel "Halt Impact"@en .

risk:HaltSource a rdfs:Class,
        skos:Concept,
        risk:RiskControl ;
    dct:contributor _:person-harshvardhan-j-pandit ;
    dct:created "2024-05-19"^^xsd:date ;
    dct:modified "2025-01-06"^^xsd:date ;
    rdfs:isDefinedBy risk: ;
    sw:term_status "modified"@en ;
    skos:broader risk:InterruptionControl,
        risk:SourceControl ;
    skos:definition "Control that halts the (ongoing) risk source event or process such that it no longer takes place or is applicable in the context"@en ;
    skos:inScheme risk:risk-controls-classes ;
    skos:prefLabel "Halt Source"@en .

risk:Harassment a rdfs:Class,
        skos:Concept,
        dpv:RiskConcept,
        risk:PotentialConsequence,
        risk:PotentialImpact,
        risk:PotentialRisk ;
    dct:created "2024-12-17"^^xsd:date ;
    rdfs:isDefinedBy risk: ;
    sw:term_status "accepted"@en ;
    skos:broader risk:Harm,
        risk:Wellbeing ;
    skos:definition "Concept representing harassment of individual(s)"@en ;
    skos:inScheme risk:risk-taxonomy-classes ;
    skos:prefLabel "Harassment"@en .

risk:Harm a rdfs:Class,
        skos:Concept,
        dpv:RiskConcept,
        risk:PotentialConsequence,
        risk:PotentialImpact,
        risk:PotentialRisk ;
    dct:contributor _:person-harshvardhan-j-pandit ;
    dct:created "2022-08-13"^^xsd:date ;
    dct:modified "2024-08-16"^^xsd:date ;
    rdfs:isDefinedBy risk: ;
    sw:term_status "accepted"@en ;
    skos:broader risk:HealthSafety,
        risk:IndividualRisk ;
    skos:definition "Concept representing Harm to humans"@en ;
    skos:inScheme risk:risk-taxonomy-classes ;
    skos:prefLabel "Harm"@en ;
    skos:scopeNote "This concept refers to the general abstract notion of harm"@en .

risk:Health a rdfs:Class,
        skos:Concept,
        dpv:RiskConcept,
        risk:PotentialConsequence,
        risk:PotentialImpact,
        risk:PotentialRisk ;
    dct:contributor _:person-harshvardhan-j-pandit ;
    dct:created "2024-12-01"^^xsd:date ;
    rdfs:isDefinedBy risk: ;
    sw:term_status "accepted"@en ;
    skos:broader risk:HealthSafety ;
    skos:definition "Concept representing health of individual(s), or group(s), or society at large"@en ;
    skos:inScheme risk:risk-taxonomy-classes ;
    skos:prefLabel "Health"@en .

risk:HealthSafety a rdfs:Class,
        skos:Concept,
        dpv:RiskConcept,
        risk:PotentialConsequence,
        risk:PotentialImpact,
        risk:PotentialRisk ;
    dct:contributor _:person-delaram-golpayegani ;
    dct:created "2024-12-01"^^xsd:date ;
    rdfs:isDefinedBy risk: ;
    sw:term_status "accepted"@en ;
    skos:broader risk:IndividualRisk ;
    skos:definition "Concept representing health & safety of individual(s), or group(s), or society at large"@en ;
    skos:inScheme risk:risk-taxonomy-classes ;
    skos:prefLabel "Health & Safety"@en .

risk:HighLikelihood a rdfs:Class,
        skos:Concept,
        dpv:Likelihood ;
    dct:contributor _:person-harshvardhan-j-pandit ;
    dct:created "2022-08-18"^^xsd:date ;
    rdf:value 0.75 ;
    rdfs:isDefinedBy risk: ;
    sw:term_status "accepted"@en ;
    skos:broader risk:3LikelihoodLevels,
        risk:5LikelihoodLevels,
        risk:7LikelihoodLevels ;
    skos:definition "Level where Likelihood is High"@en ;
    skos:inScheme risk:risk-levels-classes ;
    skos:prefLabel "High Likelihood"@en ;
    skos:scopeNote "The suggested quantitative value for this concept is 0.75 on a scale of 0 to 1"@en .

risk:HighRisk a rdfs:Class,
        skos:Concept,
        dpv:RiskLevel ;
    dct:contributor _:person-harshvardhan-j-pandit ;
    dct:created "2022-08-18"^^xsd:date ;
    rdf:value 0.75 ;
    rdfs:isDefinedBy risk: ;
    sw:term_status "accepted"@en ;
    skos:broader risk:3RiskLevels,
        risk:5RiskLevels,
        risk:7RiskLevels ;
    skos:definition "Level where Risk is High"@en ;
    skos:inScheme risk:risk-levels-classes ;
    skos:prefLabel "High Risk"@en ;
    skos:scopeNote "The suggested quantitative value for this concept is 0.75 on a scale of 0 to 1"@en .

risk:HighSeverity a rdfs:Class,
        skos:Concept,
        dpv:Severity ;
    dct:contributor _:person-harshvardhan-j-pandit ;
    dct:created "2022-08-18"^^xsd:date ;
    rdf:value 0.75 ;
    rdfs:isDefinedBy risk: ;
    sw:term_status "accepted"@en ;
    skos:broader risk:3SeverityLevels,
        risk:5SeverityLevels,
        risk:7SeverityLevels ;
    skos:definition "Level where Severity is High"@en ;
    skos:inScheme risk:risk-levels-classes ;
    skos:prefLabel "High Severity"@en ;
    skos:scopeNote "The suggested quantitative value for this concept is 0.75 on a scale of 0 to 1"@en .

risk:Homophobia a rdfs:Class,
        skos:Concept,
        dpv:RiskConcept,
        risk:PotentialConsequence,
        risk:PotentialImpact,
        risk:PotentialRisk ;
    dct:created "2024-09-30"^^xsd:date ;
    rdfs:isDefinedBy risk: ;
    sw:term_status "accepted"@en ;
    skos:broader risk:SexualOrientationDiscrimination ;
    skos:definition "Hostility or prejudice against individuals who are or are perceived to be homosexual"@en ;
    skos:inScheme risk:risk-taxonomy-classes ;
    skos:prefLabel "Homophobia"@en .

risk:HumanErrors a rdfs:Class,
        skos:Concept,
        dpv:RiskConcept,
        risk:PotentialConsequence,
        risk:PotentialRisk,
        risk:PotentialRiskSource ;
    dct:contributor _:person-harshvardhan-j-pandit ;
    dct:created "2022-08-17"^^xsd:date ;
    dct:modified "2024-08-16"^^xsd:date ;
    dct:source _:b7191aa21b975cb14bbce32aa3ba9c7eb ;
    rdfs:isDefinedBy risk: ;
    sw:term_status "accepted"@en ;
    skos:broader risk:UserRisks ;
    skos:definition "Concept representing activities that are errors caused by humans without intention and which was not caused by following rules or policies or instructions that were not from the person"@en ;
    skos:inScheme risk:risk-taxonomy-classes ;
    skos:prefLabel "Human Errors"@en .

risk:HumanOversightIneffective a rdfs:Class,
        skos:Concept,
        dpv:RiskConcept,
        risk:PotentialConsequence,
        risk:PotentialRisk,
        risk:PotentialRiskSource ;
    dct:contributor _:person-delaram-golpayegani,
        _:person-harshvardhan-j-pandit ;
    dct:created "2024-12-01"^^xsd:date ;
    rdfs:isDefinedBy risk: ;
    sw:term_status "accepted"@en ;
    skos:broader risk:OrganisationalManagementRisk ;
    skos:definition "Concept representing cases where human oversight is ineffective for the intended effect, such as for when human can observe a problem but cannot do anything about it"@en ;
    skos:inScheme risk:risk-taxonomy-classes ;
    skos:prefLabel "Human Oversight Ineffective"@en .

risk:HumanOversightInsufficient a rdfs:Class,
        skos:Concept,
        dpv:RiskConcept,
        risk:PotentialConsequence,
        risk:PotentialRisk,
        risk:PotentialRiskSource ;
    dct:contributor _:person-delaram-golpayegani,
        _:person-harshvardhan-j-pandit ;
    dct:created "2024-12-01"^^xsd:date ;
    rdfs:isDefinedBy risk: ;
    sw:term_status "accepted"@en ;
    skos:broader risk:OrganisationalManagementRisk ;
    skos:definition "Concept representing cases where human oversight is insufficient for the intended effect, such as not being capable of identifying a problem"@en ;
    skos:inScheme risk:risk-taxonomy-classes ;
    skos:prefLabel "Human Oversight Insufficient"@en .

risk:IdentificationControl a rdfs:Class,
        skos:Concept,
        risk:RiskControl ;
    dct:contributor _:person-delaram-golpayegani,
        _:person-harshvardhan-j-pandit ;
    dct:created "2024-05-19"^^xsd:date ;
    dct:modified "2025-01-06"^^xsd:date ;
    rdfs:isDefinedBy risk: ;
    sw:term_status "modified"@en ;
    skos:broader risk:MonitorControl ;
    skos:definition "Control that identifies the characteristics of an event"@en ;
    skos:inScheme risk:risk-controls-classes ;
    skos:prefLabel "Identification Control"@en ;
    skos:scopeNote "Identification in the context of an event refers to its characteristics such as likelihood, severity, as well as contextual metrics such as amount of data or power being used, or affected entities or things, and which can be used to categorise the event in terms of risk level or other contextual groupings"@en .

risk:IdentityFraud a rdfs:Class,
        skos:Concept,
        dpv:RiskConcept,
        risk:ConfidentialityConcept,
        risk:PotentialConsequence,
        risk:PotentialRisk,
        risk:PotentialRiskSource ;
    dct:contributor _:person-harshvardhan-j-pandit ;
    dct:created "2022-08-17"^^xsd:date ;
    dct:modified "2026-02-09"^^xsd:date ;
    dct:source _:b65de0d403668931587d7f38d790f5adc ;
    rdfs:isDefinedBy risk: ;
    sw:term_status "modified"@en ;
    skos:broader risk:Fraud ;
    skos:definition "Concept representing Identity Fraud"@en ;
    skos:inScheme risk:risk-taxonomy-classes ;
    skos:prefLabel "Identity Fraud"@en .

risk:IdentityTheft a rdfs:Class,
        skos:Concept,
        dpv:RiskConcept,
        risk:ConfidentialityConcept,
        risk:PotentialConsequence,
        risk:PotentialRisk,
        risk:PotentialRiskSource ;
    dct:contributor _:person-harshvardhan-j-pandit ;
    dct:created "2022-08-17"^^xsd:date ;
    dct:modified "2026-02-09"^^xsd:date ;
    dct:source _:b65de0d403668931587d7f38d790f5adc ;
    rdfs:isDefinedBy risk: ;
    sw:term_status "modified"@en ;
    skos:broader risk:MaliciousActivity ;
    skos:definition "Concept representing Identity Theft"@en ;
    skos:inScheme risk:risk-taxonomy-classes ;
    skos:prefLabel "Identity Theft"@en .

risk:IdentityVerificationFailure a rdfs:Class,
        skos:Concept,
        dpv:RiskConcept,
        risk:PotentialConsequence,
        risk:PotentialImpact,
        risk:PotentialRisk ;
    dct:created "2024-10-21"^^xsd:date ;
    rdfs:isDefinedBy risk: ;
    sw:term_status "accepted"@en ;
    skos:broader risk:ServiceRelatedConsequence ;
    skos:definition "Concept representing failure to verify identity"@en ;
    skos:inScheme risk:risk-taxonomy-classes ;
    skos:prefLabel "Identity Verification Failure"@en .

risk:IllegalDataProcessing a rdfs:Class,
        skos:Concept,
        dpv:RiskConcept,
        risk:PotentialConsequence,
        risk:PotentialRisk ;
    dct:contributor _:person-harshvardhan-j-pandit ;
    dct:created "2022-08-17"^^xsd:date ;
    dct:modified "2024-08-16"^^xsd:date ;
    dct:source _:b15886bc6e88dcdb258fe59ded7be3abf ;
    rdfs:isDefinedBy risk: ;
    sw:term_status "accepted"@en ;
    skos:broader risk:LegalComplianceRisk ;
    skos:definition "Concept representing Illegal Processing of Data"@en ;
    skos:inScheme risk:risk-taxonomy-classes ;
    skos:prefLabel "Illegal Data Processing"@en ;
    skos:scopeNote "This concept was called \"IllegalProcessingData\" in DPV 2.0"@en .

risk:ImpactControl a rdfs:Class,
        skos:Concept,
        risk:RiskControl ;
    dct:contributor _:person-harshvardhan-j-pandit ;
    dct:created "2024-05-19"^^xsd:date ;
    dct:modified "2025-01-06"^^xsd:date ;
    rdfs:isDefinedBy risk: ;
    sw:term_status "modified"@en ;
    skos:broader risk:RiskControl ;
    skos:definition "Risk Mitigation Measure that controls Impacts"@en ;
    skos:inScheme risk:risk-controls-classes ;
    skos:prefLabel "Impact Control"@en .

risk:ImpairedDecisionMaking a rdfs:Class,
        skos:Concept,
        dpv:RiskConcept,
        risk:PotentialConsequence,
        risk:PotentialImpact,
        risk:PotentialRisk ;
    dct:contributor _:person-delaram-golpayegani,
        _:person-harshvardhan-j-pandit ;
    dct:created "2026-02-09"^^xsd:date ;
    rdfs:isDefinedBy risk: ;
    sw:term_status "accepted"@en ;
    skos:broader risk:IndividualRisk ;
    skos:definition "Concept representing Impaired Decision Making"@en ;
    skos:inScheme risk:risk-taxonomy-classes ;
    skos:prefLabel "Impaired Decision Making"@en .

risk:ImplicitBias a rdfs:Class,
        skos:Concept,
        dpv:RiskConcept,
        risk:PotentialConsequence,
        risk:PotentialRisk,
        risk:PotentialRiskSource ;
    dct:contributor _:person-daniel-doherty,
        _:person-delaram-golpayegani,
        _:person-harshvardhan-j-pandit ;
    dct:created "2024-09-13"^^xsd:date ;
    dct:source "ISO/IEC 24027:2021"@en ;
    rdfs:isDefinedBy risk: ;
    sw:term_status "accepted"@en ;
    skos:broader risk:CognitiveBias ;
    skos:definition "Bias that occurs when a human makes an association or assumption based on their mental models and memories"@en ;
    skos:inScheme risk:risk-taxonomy-classes ;
    skos:prefLabel "Implicit Bias"@en .

risk:InGroupBias a rdfs:Class,
        skos:Concept,
        dpv:RiskConcept,
        risk:PotentialConsequence,
        risk:PotentialRisk,
        risk:PotentialRiskSource ;
    dct:contributor _:person-daniel-doherty,
        _:person-delaram-golpayegani,
        _:person-harshvardhan-j-pandit ;
    dct:created "2024-09-13"^^xsd:date ;
    dct:source "ISO/IEC 24027:2021"@en ;
    rdfs:isDefinedBy risk: ;
    sw:term_status "accepted"@en ;
    skos:broader risk:CognitiveBias ;
    skos:definition "Bias that occurs when showing partiality to one's own group or own characteristics"@en ;
    skos:inScheme risk:risk-taxonomy-classes ;
    skos:prefLabel "In-Group Bias"@en .

risk:InabilityToEnterIntoContract a rdfs:Class,
        skos:Concept,
        dpv:RiskConcept,
        risk:PotentialConsequence,
        risk:PotentialImpact,
        risk:PotentialRisk ;
    dct:created "2024-10-21"^^xsd:date ;
    rdfs:isDefinedBy risk: ;
    sw:term_status "accepted"@en ;
    skos:broader risk:ServiceRelatedConsequence ;
    skos:definition "Concept representing inability to enter into contract"@en ;
    skos:inScheme risk:risk-taxonomy-classes ;
    skos:prefLabel "Inability to Enter Into Contract"@en .

risk:InabilityToEstablishLegalClaims a rdfs:Class,
        skos:Concept,
        dpv:RiskConcept,
        risk:PotentialConsequence,
        risk:PotentialImpact,
        risk:PotentialRisk ;
    dct:created "2024-10-21"^^xsd:date ;
    rdfs:isDefinedBy risk: ;
    sw:term_status "accepted"@en ;
    skos:broader risk:ServiceRelatedConsequence ;
    skos:definition "Concept representing inability to establish legal claims"@en ;
    skos:inScheme risk:risk-taxonomy-classes ;
    skos:prefLabel "Inability to Establish Legal Claims"@en .

risk:InabilityToFulfilLegalObligations a rdfs:Class,
        skos:Concept,
        dpv:RiskConcept,
        risk:PotentialConsequence,
        risk:PotentialImpact,
        risk:PotentialRisk ;
    dct:contributor _:person-arthit-suriyawongkul,
        _:person-harshvardhan-j-pandit ;
    dct:created "2024-10-21"^^xsd:date ;
    dct:modified "2025-08-06"^^xsd:date ;
    rdfs:isDefinedBy risk: ;
    sw:term_status "modified"@en ;
    skos:broader risk:ServiceRelatedConsequence ;
    skos:definition "Concept representing inability to fulfil legal obligations"@en ;
    skos:inScheme risk:risk-taxonomy-classes ;
    skos:prefLabel "Inability to Fulfil Legal Obligations"@en .

risk:InabilityToProcessPayments a rdfs:Class,
        skos:Concept,
        dpv:RiskConcept,
        risk:PotentialConsequence,
        risk:PotentialImpact,
        risk:PotentialRisk ;
    dct:created "2024-10-21"^^xsd:date ;
    rdfs:isDefinedBy risk: ;
    sw:term_status "accepted"@en ;
    skos:broader risk:ServiceRelatedConsequence ;
    skos:definition "Concept representing inability to process payments"@en ;
    skos:inScheme risk:risk-taxonomy-classes ;
    skos:prefLabel "Inability to Process Payments"@en .

risk:InabilityToProtectVitalInterests a rdfs:Class,
        skos:Concept,
        dpv:RiskConcept,
        risk:PotentialConsequence,
        risk:PotentialImpact,
        risk:PotentialRisk ;
    dct:created "2024-10-21"^^xsd:date ;
    rdfs:isDefinedBy risk: ;
    sw:term_status "accepted"@en ;
    skos:broader risk:ServiceRelatedConsequence ;
    skos:definition "Concept representing inability to protect vital interests"@en ;
    skos:inScheme risk:risk-taxonomy-classes ;
    skos:prefLabel "Inability to Protect Vital Interests"@en .

risk:InabilityToProvideHealthCare a rdfs:Class,
        skos:Concept,
        dpv:RiskConcept,
        risk:PotentialConsequence,
        risk:PotentialImpact,
        risk:PotentialRisk ;
    dct:created "2024-10-21"^^xsd:date ;
    rdfs:isDefinedBy risk: ;
    sw:term_status "accepted"@en ;
    skos:broader risk:ServiceRelatedConsequence ;
    skos:definition "Concept representing inability to provide health care"@en ;
    skos:inScheme risk:risk-taxonomy-classes ;
    skos:prefLabel "Inability to Provide Health Care"@en .

risk:Incident a rdfs:Class,
        skos:Concept ;
    dct:contributor _:person-delaram-golpayegani,
        _:person-harshvardhan-j-pandit,
        _:person-julio-hernandez,
        _:person-rob-brennan ;
    dct:created "2024-02-14"^^xsd:date ;
    dct:modified "2024-08-16"^^xsd:date ;
    vann:example dex:E0069,
        dex:E0070 ;
    rdfs:isDefinedBy risk: ;
    rdfs:subClassOf dpv:RiskConcept ;
    sw:term_status "accepted"@en ;
    skos:broader dpv:RiskConcept ;
    skos:definition "An actual or occurred event"@en ;
    skos:inScheme risk:incident-classes ;
    skos:prefLabel "Incident"@en ;
    skos:scopeNote "Incident is realised or materialised risk"@en .

risk:IncidentAssessmentReport a rdfs:Class,
        skos:Concept ;
    dct:created "2024-05-19"^^xsd:date ;
    rdfs:isDefinedBy risk: ;
    rdfs:subClassOf risk:IncidentReport ;
    sw:term_status "accepted"@en ;
    skos:broader risk:IncidentReport ;
    skos:definition "A report describing the assessment of an incident in terms of its effects or impacts"@en ;
    skos:inScheme risk:incident-classes ;
    skos:prefLabel "Incident Assessment Report"@en .

risk:IncidentConcluded a rdfs:Class,
        skos:Concept,
        risk:IncidentStatus ;
    dct:contributor _:person-harshvardhan-j-pandit ;
    dct:created "2024-02-14"^^xsd:date ;
    rdfs:isDefinedBy risk: ;
    sw:term_status "accepted"@en ;
    skos:broader risk:IncidentStatus ;
    skos:definition "The incident has stopped or finished or concluded without any active mitigation and with a low likelihood of resuming or recurring"@en ;
    skos:inScheme risk:incident-status-classes ;
    skos:prefLabel "Incident Concluded"@en .

risk:IncidentConcludingReport a rdfs:Class,
        skos:Concept ;
    dct:created "2024-05-19"^^xsd:date ;
    rdfs:isDefinedBy risk: ;
    rdfs:subClassOf risk:IncidentReport ;
    sw:term_status "accepted"@en ;
    skos:broader risk:IncidentReport ;
    skos:definition "A report describing the conclusion of an investigation regarding an incident where all relevant facts are known"@en ;
    skos:inScheme risk:incident-classes ;
    skos:prefLabel "Incident Concluding Report"@en .

risk:IncidentDetectionReport a rdfs:Class,
        skos:Concept ;
    dct:created "2024-05-19"^^xsd:date ;
    rdfs:isDefinedBy risk: ;
    rdfs:subClassOf risk:IncidentReport ;
    sw:term_status "accepted"@en ;
    skos:broader risk:IncidentReport ;
    skos:definition "A report describing the detection of an incident"@en ;
    skos:inScheme risk:incident-classes ;
    skos:prefLabel "Incident Detection Report"@en .

risk:IncidentHalted a rdfs:Class,
        skos:Concept,
        risk:IncidentStatus ;
    dct:contributor _:person-harshvardhan-j-pandit ;
    dct:created "2024-02-14"^^xsd:date ;
    rdfs:isDefinedBy risk: ;
    sw:term_status "accepted"@en ;
    skos:broader risk:IncidentStatus ;
    skos:definition "The incident has halted or paused with a high likelihood of resuming or recurring"@en ;
    skos:inScheme risk:incident-status-classes ;
    skos:prefLabel "Incident Halted"@en .

risk:IncidentHandlingReport a rdfs:Class,
        skos:Concept ;
    dct:created "2024-05-19"^^xsd:date ;
    rdfs:isDefinedBy risk: ;
    rdfs:subClassOf risk:IncidentReport ;
    sw:term_status "accepted"@en ;
    skos:broader risk:IncidentReport ;
    skos:definition "A report describing the response to or handling of an incident regarding the mitigation of its effects and the prevention of its recurrence"@en ;
    skos:inScheme risk:incident-classes ;
    skos:prefLabel "Incident Handling Report"@en .

risk:IncidentIdentifier a rdfs:Class,
        skos:Concept ;
    dct:created "2024-05-19"^^xsd:date ;
    rdfs:isDefinedBy risk: ;
    rdfs:subClassOf rdfs:Class ;
    sw:term_status "accepted"@en ;
    skos:definition "Identifier associated with an incident"@en ;
    skos:inScheme risk:incident-classes ;
    skos:prefLabel "Incident Identifier"@en .

risk:IncidentImpactAssessment a rdfs:Class,
        skos:Concept ;
    dct:contributor _:person-harshvardhan-j-pandit ;
    dct:created "2024-05-19"^^xsd:date ;
    rdfs:isDefinedBy risk: ;
    rdfs:subClassOf dpv:ImpactAssessment ;
    sw:term_status "accepted"@en ;
    skos:broader dpv:ImpactAssessment ;
    skos:definition "An impact assessment associated with an incident"@en ;
    skos:inScheme risk:incident-classes ;
    skos:prefLabel "Incident Impact Assessment"@en .

risk:IncidentInvestigationCompleted a rdfs:Class,
        skos:Concept,
        risk:IncidentInvestigationStatus ;
    dct:contributor _:person-harshvardhan-j-pandit ;
    dct:created "2024-12-01"^^xsd:date ;
    rdfs:isDefinedBy risk: ;
    sw:term_status "accepted"@en ;
    skos:broader risk:IncidentInvestigationStatus ;
    skos:definition "Status indicating the investigation has been completed and findings are available"@en ;
    skos:inScheme risk:incident-status-classes ;
    skos:prefLabel "Incident Investigation Completed"@en .

risk:IncidentInvestigationNotStarted a rdfs:Class,
        skos:Concept,
        risk:IncidentInvestigationStatus ;
    dct:contributor _:person-harshvardhan-j-pandit ;
    dct:created "2024-12-01"^^xsd:date ;
    rdfs:isDefinedBy risk: ;
    sw:term_status "accepted"@en ;
    skos:broader risk:IncidentInvestigationStatus ;
    skos:definition "Status indicating the investigation has not yet been started"@en ;
    skos:inScheme risk:incident-status-classes ;
    skos:prefLabel "Incident Investigation Not Started"@en .

risk:IncidentInvestigationOngoing a rdfs:Class,
        skos:Concept,
        risk:IncidentInvestigationStatus ;
    dct:contributor _:person-harshvardhan-j-pandit ;
    dct:created "2024-12-01"^^xsd:date ;
    rdfs:isDefinedBy risk: ;
    sw:term_status "accepted"@en ;
    skos:broader risk:IncidentInvestigationStatus ;
    skos:definition "Status indicating the investigation is ongoing"@en ;
    skos:inScheme risk:incident-status-classes ;
    skos:prefLabel "Incident Investigation Ongoing"@en .

risk:IncidentInvestigationPreliminary a rdfs:Class,
        skos:Concept,
        risk:IncidentInvestigationStatus ;
    dct:contributor _:person-harshvardhan-j-pandit ;
    dct:created "2024-12-01"^^xsd:date ;
    rdfs:isDefinedBy risk: ;
    sw:term_status "accepted"@en ;
    skos:broader risk:IncidentInvestigationStatus ;
    skos:definition "Status indicating the investigation is at a preliminary stage with limited findings"@en ;
    skos:inScheme risk:incident-status-classes ;
    skos:prefLabel "Incident Investigation Preliminary"@en .

risk:IncidentInvestigationStatus a rdfs:Class,
        skos:Concept ;
    dct:contributor _:person-harshvardhan-j-pandit ;
    dct:created "2024-12-01"^^xsd:date ;
    rdfs:isDefinedBy risk: ;
    rdfs:subClassOf dpv:Status ;
    sw:term_status "accepted"@en ;
    skos:broader dpv:Status ;
    skos:definition "Status associated with investigation of an incident"@en ;
    skos:inScheme risk:incident-status-classes ;
    skos:prefLabel "Incident Investigation Status"@en .

risk:IncidentMitigated a rdfs:Class,
        skos:Concept,
        risk:IncidentStatus ;
    dct:contributor _:person-harshvardhan-j-pandit ;
    dct:created "2024-02-14"^^xsd:date ;
    rdfs:isDefinedBy risk: ;
    sw:term_status "accepted"@en ;
    skos:broader risk:IncidentStatus ;
    skos:definition "The incident has been mitigated against future recurrences i.e. a measure has been applied to prevent the same or similar incident from recurring"@en ;
    skos:inScheme risk:incident-status-classes ;
    skos:prefLabel "Incident Mitigated"@en .

risk:IncidentMitigationMeasure a rdfs:Class,
        skos:Concept ;
    dct:created "2024-05-19"^^xsd:date ;
    rdfs:isDefinedBy risk: ;
    rdfs:subClassOf dpv:RiskMitigationMeasure ;
    sw:term_status "accepted"@en ;
    skos:broader dpv:RiskMitigationMeasure ;
    skos:definition "A mitigation measure taken in response specifically to mitigate an incident and prevent it from occurring again"@en ;
    skos:inScheme risk:incident-classes ;
    skos:prefLabel "Incident Mitigation Measure"@en .

risk:IncidentNearMiss a rdfs:Class,
        skos:Concept,
        risk:IncidentStatus ;
    dct:contributor _:person-harshvardhan-j-pandit ;
    dct:created "2024-02-14"^^xsd:date ;
    rdfs:isDefinedBy risk: ;
    sw:term_status "accepted"@en ;
    skos:broader risk:IncidentStatus ;
    skos:definition "The state where an incident was almost successful in taking place i.e. \"it came very close\""@en ;
    skos:inScheme risk:incident-status-classes ;
    skos:prefLabel "Incident Near Miss"@en .

risk:IncidentNotice a rdfs:Class,
        skos:Concept ;
    dct:created "2024-05-19"^^xsd:date ;
    rdfs:isDefinedBy risk: ;
    rdfs:subClassOf dpv:Notice ;
    sw:term_status "accepted"@en ;
    skos:broader dpv:Notice ;
    skos:definition "Notice associated with an incident"@en ;
    skos:inScheme risk:incident-classes ;
    skos:prefLabel "Incident Notice"@en .

risk:IncidentOngoing a rdfs:Class,
        skos:Concept,
        risk:IncidentStatus ;
    dct:contributor _:person-harshvardhan-j-pandit ;
    dct:created "2024-02-14"^^xsd:date ;
    rdfs:isDefinedBy risk: ;
    sw:term_status "accepted"@en ;
    skos:broader risk:IncidentStatus ;
    skos:definition "The incident is ongoing i.e. still active"@en ;
    skos:inScheme risk:incident-status-classes ;
    skos:prefLabel "Incident Ongoing"@en .

risk:IncidentOngoingReport a rdfs:Class,
        skos:Concept ;
    dct:created "2024-05-19"^^xsd:date ;
    rdfs:isDefinedBy risk: ;
    rdfs:subClassOf risk:IncidentReport ;
    sw:term_status "accepted"@en ;
    skos:broader risk:IncidentReport ;
    skos:definition "A report describing on ongoing investigation regarding an incident where facts and extent of the investigation are being investigated"@en ;
    skos:inScheme risk:incident-classes ;
    skos:prefLabel "Incident Ongoing Report"@en .

risk:IncidentPreliminaryReport a rdfs:Class,
        skos:Concept ;
    dct:created "2024-05-19"^^xsd:date ;
    rdfs:isDefinedBy risk: ;
    rdfs:subClassOf risk:IncidentReport ;
    sw:term_status "accepted"@en ;
    skos:broader risk:IncidentReport ;
    skos:definition "A report describing the preliminary investigation regarding an incident where the complete facts or extent of the incident may not be known"@en ;
    skos:inScheme risk:incident-classes ;
    skos:prefLabel "Incident Preliminary Report"@en .

risk:IncidentRegister a rdfs:Class,
        skos:Concept ;
    dct:contributor _:person-harshvardhan-j-pandit ;
    dct:created "2024-05-19"^^xsd:date ;
    rdfs:isDefinedBy risk: ;
    rdfs:subClassOf dpv:RecordsOfActivities ;
    sw:term_status "accepted"@en ;
    skos:broader dpv:RecordsOfActivities ;
    skos:definition "A register recording incidents, their reports, notifications, and other related activities"@en ;
    skos:inScheme risk:incident-classes ;
    skos:prefLabel "Incident Register"@en .

risk:IncidentReport a rdfs:Class,
        skos:Concept ;
    dct:created "2024-05-19"^^xsd:date ;
    rdfs:isDefinedBy risk: ;
    rdfs:subClassOf dpv:RecordsOfActivities ;
    sw:term_status "accepted"@en ;
    skos:broader dpv:RecordsOfActivities ;
    skos:definition "Documented information about an incident, its handling, assessments,and notifications"@en ;
    skos:inScheme risk:incident-classes ;
    skos:prefLabel "Incident Report"@en .

risk:IncidentStatus a rdfs:Class,
        skos:Concept ;
    dct:contributor _:person-harshvardhan-j-pandit ;
    dct:created "2024-02-14"^^xsd:date ;
    vann:example dex:E0069 ;
    rdfs:isDefinedBy risk: ;
    rdfs:subClassOf dpv:Status ;
    sw:term_status "accepted"@en ;
    skos:broader dpv:Status ;
    skos:definition "Status associated with an incident"@en ;
    skos:inScheme risk:incident-status-classes ;
    skos:prefLabel "Incident Status"@en .

risk:IncidentStatusUnknown a rdfs:Class,
        skos:Concept,
        risk:IncidentStatus ;
    dct:contributor _:person-harshvardhan-j-pandit ;
    dct:created "2024-02-14"^^xsd:date ;
    rdfs:isDefinedBy risk: ;
    sw:term_status "accepted"@en ;
    skos:broader risk:IncidentStatus ;
    skos:definition "The status of a incident is unknown"@en ;
    skos:inScheme risk:incident-status-classes ;
    skos:prefLabel "Incident Status Unknown"@en .

risk:IncidentSuspected a rdfs:Class,
        skos:Concept,
        risk:IncidentStatus ;
    dct:contributor _:person-harshvardhan-j-pandit ;
    dct:created "2024-02-14"^^xsd:date ;
    rdfs:isDefinedBy risk: ;
    sw:term_status "accepted"@en ;
    skos:broader risk:IncidentStatus ;
    skos:definition "The state where a incident is suspected, but has not yet been confirmed. This can be due to lack of information, or because the process of detection and investigation is still ongoing"@en ;
    skos:inScheme risk:incident-status-classes ;
    skos:prefLabel "Incident Suspected"@en .

risk:IncidentSuspectedReport a rdfs:Class,
        skos:Concept ;
    dct:created "2024-05-19"^^xsd:date ;
    rdfs:isDefinedBy risk: ;
    rdfs:subClassOf risk:IncidentReport ;
    sw:term_status "accepted"@en ;
    skos:broader risk:IncidentReport ;
    skos:definition "A report describing the suspicion of an incident in the past or occurring"@en ;
    skos:inScheme risk:incident-classes ;
    skos:prefLabel "Incident Suspected Report"@en .

risk:IncidentTerminated a rdfs:Class,
        skos:Concept,
        risk:IncidentStatus ;
    dct:contributor _:person-harshvardhan-j-pandit ;
    dct:created "2024-02-14"^^xsd:date ;
    rdfs:isDefinedBy risk: ;
    sw:term_status "accepted"@en ;
    skos:broader risk:IncidentStatus ;
    skos:definition "The incident has been stopped or terminated through the use of a mitigation or deterrent measure with a low likelihood of resuming or recurring"@en ;
    skos:inScheme risk:incident-status-classes ;
    skos:prefLabel "Incident Terminated"@en .

risk:IndirectDiscrimination a rdfs:Class,
        skos:Concept,
        dpv:RiskConcept,
        risk:PotentialConsequence,
        risk:PotentialImpact,
        risk:PotentialRisk ;
    dct:created "2024-09-30"^^xsd:date ;
    rdfs:isDefinedBy risk: ;
    sw:term_status "accepted"@en ;
    skos:broader risk:Discrimination ;
    skos:definition "Occurs when an apparently neutral provision, criterion, or practice puts individuals of a certain group at a disadvantage compared to others, unless it can be objectively justified"@en ;
    skos:inScheme risk:risk-taxonomy-classes ;
    skos:prefLabel "Indirect Discrimination"@en .

risk:IndividualHealthSafety a rdfs:Class,
        skos:Concept,
        dpv:RiskConcept,
        risk:PotentialConsequence,
        risk:PotentialImpact,
        risk:PotentialRisk ;
    dct:created "2022-08-17"^^xsd:date ;
    dct:modified "2024-12-01"^^xsd:date ;
    rdfs:isDefinedBy risk: ;
    sw:term_status "modified"@en ;
    skos:broader risk:HealthSafety,
        risk:IndividualRisk ;
    skos:definition "Concept representing health & safety of individual(s)"@en ;
    skos:inScheme risk:risk-taxonomy-classes ;
    skos:prefLabel "Individual Health & Safety"@en .

risk:IndividualRisk a rdfs:Class,
        skos:Concept,
        dpv:RiskConcept,
        risk:PotentialConsequence,
        risk:PotentialImpact,
        risk:PotentialRisk ;
    dct:created "2024-12-17"^^xsd:date ;
    rdfs:isDefinedBy risk: ;
    sw:term_status "accepted"@en ;
    skos:broader risk:SocietalRiskConcept ;
    skos:definition "Risks and issues that affect or have the potential to affect specific individuals"@en ;
    skos:inScheme risk:risk-taxonomy-classes ;
    skos:prefLabel "Individual Risk"@en .

risk:InformativenessBias a rdfs:Class,
        skos:Concept,
        dpv:RiskConcept,
        risk:PotentialConsequence,
        risk:PotentialRisk,
        risk:PotentialRiskSource ;
    dct:contributor _:person-daniel-doherty,
        _:person-delaram-golpayegani,
        _:person-harshvardhan-j-pandit ;
    dct:created "2024-09-13"^^xsd:date ;
    dct:source "ISO/IEC 24027:2021"@en ;
    rdfs:isDefinedBy risk: ;
    sw:term_status "accepted"@en ;
    skos:broader risk:DataBias ;
    skos:definition "Bias that occurs when the mapping between inputs present in the data and outputs are more difficult to identify for some group"@en ;
    skos:inScheme risk:risk-taxonomy-classes ;
    skos:prefLabel "Informativeness Bias"@en .

risk:Injury a rdfs:Class,
        skos:Concept,
        dpv:RiskConcept,
        risk:PotentialConsequence,
        risk:PotentialImpact,
        risk:PotentialRisk ;
    dct:contributor _:person-harshvardhan-j-pandit ;
    dct:created "2022-08-17"^^xsd:date ;
    dct:modified "2024-08-16"^^xsd:date ;
    dct:source _:b15886bc6e88dcdb258fe59ded7be3abf ;
    rdfs:isDefinedBy risk: ;
    sw:term_status "accepted"@en ;
    skos:broader risk:Harm,
        risk:PhysicalSafety ;
    skos:definition "Concept representing Injury"@en ;
    skos:inScheme risk:risk-taxonomy-classes ;
    skos:prefLabel "Injury"@en .

risk:InstructionsInaccessible a rdfs:Class,
        skos:Concept,
        dpv:RiskConcept,
        risk:PotentialConsequence,
        risk:PotentialRisk,
        risk:PotentialRiskSource ;
    dct:contributor _:person-delaram-golpayegani ;
    dct:created "2026-02-09"^^xsd:date ;
    rdfs:isDefinedBy risk: ;
    sw:term_status "accepted"@en ;
    skos:broader risk:DocumentationIssues ;
    skos:definition "Concept representing cases wher instructions are inaccessible"@en ;
    skos:inScheme risk:risk-taxonomy-classes ;
    skos:prefLabel "Instructions Inaccessible"@en .

risk:InstructionsIncorrect a rdfs:Class,
        skos:Concept,
        dpv:RiskConcept,
        risk:PotentialConsequence,
        risk:PotentialRisk,
        risk:PotentialRiskSource ;
    dct:contributor _:person-delaram-golpayegani,
        _:person-harshvardhan-j-pandit ;
    dct:created "2024-12-01"^^xsd:date ;
    dct:modified "2026-02-09"^^xsd:date ;
    rdfs:isDefinedBy risk: ;
    sw:term_status "modified"@en ;
    skos:broader risk:DocumentationIssues ;
    skos:definition "Concept representing cases where instructions are incorrect for achieving the intended effect"@en ;
    skos:inScheme risk:risk-taxonomy-classes ;
    skos:prefLabel "Instructions Incorrect"@en .

risk:InstructionsInsufficient a rdfs:Class,
        skos:Concept,
        dpv:RiskConcept,
        risk:PotentialConsequence,
        risk:PotentialRisk,
        risk:PotentialRiskSource ;
    dct:contributor _:person-delaram-golpayegani,
        _:person-harshvardhan-j-pandit ;
    dct:created "2024-12-01"^^xsd:date ;
    dct:modified "2026-02-09"^^xsd:date ;
    rdfs:isDefinedBy risk: ;
    sw:term_status "modified"@en ;
    skos:broader risk:DocumentationIssues ;
    skos:definition "Concept representing cases where instructions are not sufficient for the intended effect"@en ;
    skos:inScheme risk:risk-taxonomy-classes ;
    skos:prefLabel "Instructions Insufficient"@en .

risk:InstructionsUnsuitable a rdfs:Class,
        skos:Concept,
        dpv:RiskConcept,
        risk:PotentialConsequence,
        risk:PotentialRisk,
        risk:PotentialRiskSource ;
    dct:contributor _:person-delaram-golpayegani ;
    dct:created "2026-02-09"^^xsd:date ;
    rdfs:isDefinedBy risk: ;
    sw:term_status "accepted"@en ;
    skos:broader risk:DocumentationIssues ;
    skos:definition "Concept representing cases wher instructions are unsuitable for the specific task or for the specific audience, including due to incomprehensibility, lack of knowledge, or not being fit for purpose"@en ;
    skos:inScheme risk:risk-taxonomy-classes ;
    skos:prefLabel "Instructions Unsuitable"@en .

risk:IntegrityBreach a rdfs:Class,
        skos:Concept,
        dpv:RiskConcept,
        risk:IntegrityConcept,
        risk:PotentialConsequence,
        risk:PotentialRisk,
        risk:PotentialRiskSource ;
    dct:created "2024-12-17"^^xsd:date ;
    rdfs:isDefinedBy risk: ;
    sw:term_status "accepted"@en ;
    skos:broader risk:DataBreach ;
    skos:definition "Concept representing a breach of integrity"@en ;
    skos:inScheme risk:risk-taxonomy-classes ;
    skos:prefLabel "Integrity Breach"@en .

risk:IntegrityConcept a rdfs:Class,
        skos:Concept ;
    dct:contributor _:person-harshvardhan-j-pandit ;
    dct:created "2024-09-29"^^xsd:date ;
    rdfs:isDefinedBy risk: ;
    rdfs:subClassOf dpv:RiskConcept ;
    sw:term_status "accepted"@en ;
    skos:broader dpv:RiskConcept ;
    skos:definition "Indicates a concept is relevant to 'Integrity' in CIA InfoSec model"@en ;
    skos:inScheme risk:risk-taxonomy-classes ;
    skos:prefLabel "Integrity Concept"@en ;
    skos:scopeNote "This concept allows indicating the applicability of Integrity dimension to concepts whether they are a risk source, risk, consequence, or impact"@en .

risk:IntegrityIncident a rdfs:Class,
        skos:Concept ;
    dct:created "2024-05-19"^^xsd:date ;
    rdfs:isDefinedBy risk: ;
    rdfs:subClassOf risk:Incident ;
    sw:term_status "accepted"@en ;
    skos:broader risk:Incident ;
    skos:definition "Incident where the integrity of information or system has been affected"@en ;
    skos:inScheme risk:incident-classes ;
    skos:prefLabel "Integrity Incident"@en .

risk:IntentionalManipulation a rdfs:Class,
        skos:Concept,
        dpv:RiskConcept,
        risk:ConfidentialityConcept,
        risk:IntegrityConcept,
        risk:PotentialConsequence,
        risk:PotentialRisk,
        risk:PotentialRiskSource ;
    dct:contributor _:person-delaram-golpayegani ;
    dct:created "2026-02-09"^^xsd:date ;
    rdfs:isDefinedBy risk: ;
    sw:term_status "accepted"@en ;
    skos:broader risk:MaliciousActivity ;
    skos:definition "Concept representing Intentional Manipulation"@en ;
    skos:inScheme risk:risk-taxonomy-classes ;
    skos:prefLabel "Intentional Manipulation"@en .

risk:IntentionalMisuse a rdfs:Class,
        skos:Concept,
        dpv:RiskConcept,
        risk:PotentialConsequence,
        risk:PotentialRisk,
        risk:PotentialRiskSource ;
    dct:created "2024-12-17"^^xsd:date ;
    rdfs:isDefinedBy risk: ;
    sw:term_status "accepted"@en ;
    skos:broader risk:Misuse ;
    skos:definition "Concept represent an intentional misuse (of something)"@en ;
    skos:inScheme risk:risk-taxonomy-classes ;
    skos:prefLabel "Intentional Misuse"@en .

risk:InterceptCommunications a rdfs:Class,
        skos:Concept,
        dpv:RiskConcept,
        risk:ConfidentialityConcept,
        risk:PotentialConsequence,
        risk:PotentialRisk,
        risk:PotentialRiskSource ;
    dct:contributor _:person-harshvardhan-j-pandit ;
    dct:created "2022-08-17"^^xsd:date ;
    dct:modified "2024-08-16"^^xsd:date ;
    dct:source _:b15886bc6e88dcdb258fe59ded7be3abf ;
    rdfs:isDefinedBy risk: ;
    sw:term_status "modified"@en ;
    skos:broader risk:MaliciousActivity ;
    skos:definition "Concept representing Interception of Communications"@en ;
    skos:inScheme risk:risk-taxonomy-classes ;
    skos:prefLabel "Intercept Communications"@en ;
    skos:scopeNote "This concept was called \"InterceptionCommunications\" in DPV 2.0"@en .

risk:InterruptionControl a rdfs:Class,
        skos:Concept,
        risk:RiskControl ;
    dct:contributor _:person-delaram-golpayegani,
        _:person-harshvardhan-j-pandit ;
    dct:created "2025-01-06"^^xsd:date ;
    rdfs:isDefinedBy risk: ;
    sw:term_status "accepted"@en ;
    skos:broader risk:ReductionControl ;
    skos:definition "Control that interrupts an event without removing the possibility for it to be resumed and where the aim is to stop the event"@en ;
    skos:inScheme risk:risk-controls-classes ;
    skos:prefLabel "Interruption Control"@en ;
    skos:scopeNote "Interruption refers to the event being temporarily halted, such as an emergency measure while further suitable measures are identified and put in place. To indicate stopping the event completely rather than a temporary interruption, see risk:RemediationControl which fixes the underlying issue and risk:EliminationControl which prevents the event from occurring"@en .

risk:InterventionControl a rdfs:Class,
        skos:Concept,
        risk:RiskControl ;
    dct:contributor _:person-harshvardhan-j-pandit ;
    dct:created "2025-01-06"^^xsd:date ;
    rdfs:isDefinedBy risk: ;
    sw:term_status "accepted"@en ;
    skos:broader risk:ReductionControl ;
    skos:definition "Control that intervenes in the operations of the event to change some context with the aim of changing the event or the effects"@en ;
    skos:inScheme risk:risk-controls-classes ;
    skos:prefLabel "Intervention Control"@en ;
    skos:scopeNote "Intervention implies taking steps to resolve the effects or to prevent further escalation while the event is still ongoing. For halting the event, see risk:InterruptionControl, for recovering and undoing the effects, see risk:RecoveryControl and risk:ReversalControl. Intervention is a temporary or stop-gap measure which is used while the event is ongoing to prevent it from escalating or creating additional issues"@en .

risk:InvestigationControl a rdfs:Class,
        skos:Concept,
        risk:RiskControl ;
    dct:contributor _:person-harshvardhan-j-pandit ;
    dct:created "2025-01-06"^^xsd:date ;
    rdfs:isDefinedBy risk: ;
    sw:term_status "accepted"@en ;
    skos:broader risk:ReactiveControl ;
    skos:definition "Control that identifies information through an investigative process about an event and its effects after it has occurred"@en ;
    skos:inScheme risk:risk-controls-classes ;
    skos:prefLabel "Investigation Control"@en ;
    skos:scopeNote "Investigative controls are used to identify information about an event and its effects which can be used to identify further effective measures to address them, and to identify processes to remedy and recover from it. Investigation control therefore is focused on analysis of an event after its occurrence with the goal of identifying applicability and effectiveness of other controls to address it"@en .

risk:JudicialCosts a rdfs:Class,
        skos:Concept,
        dpv:RiskConcept,
        risk:PotentialConsequence,
        risk:PotentialImpact,
        risk:PotentialRisk ;
    dct:created "2024-12-17"^^xsd:date ;
    rdfs:isDefinedBy risk: ;
    sw:term_status "accepted"@en ;
    skos:broader risk:FinancialLoss ;
    skos:definition "Something that involves or causes judicial costs to be paid"@en ;
    skos:inScheme risk:risk-taxonomy-classes ;
    skos:prefLabel "Judicial Costs"@en .

risk:JudicialPenalty a rdfs:Class,
        skos:Concept,
        dpv:RiskConcept,
        risk:PotentialConsequence,
        risk:PotentialImpact,
        risk:PotentialRisk ;
    dct:created "2024-12-17"^^xsd:date ;
    rdfs:isDefinedBy risk: ;
    sw:term_status "accepted"@en ;
    skos:broader risk:FinancialLoss ;
    skos:definition "Something that involves or causes judicial penalties to be paid"@en ;
    skos:inScheme risk:risk-taxonomy-classes ;
    skos:prefLabel "Judicial Penalty"@en .

risk:LackOfSystemTransparency a rdfs:Class,
        skos:Concept,
        dpv:RiskConcept,
        risk:PotentialConsequence,
        risk:PotentialRisk,
        risk:PotentialRiskSource ;
    dct:contributor _:person-delaram-golpayegani,
        _:person-harshvardhan-j-pandit ;
    dct:created "2024-12-01"^^xsd:date ;
    rdfs:isDefinedBy risk: ;
    sw:term_status "accepted"@en ;
    skos:broader risk:OrganisationalManagementRisk ;
    skos:definition "Concept representing lack of transparency to humans related to the operation of a system"@en ;
    skos:inScheme risk:risk-taxonomy-classes ;
    skos:prefLabel "Lack Of System Transparency"@en .

risk:LanguageDiscrimination a rdfs:Class,
        skos:Concept,
        dpv:RiskConcept,
        risk:PotentialConsequence,
        risk:PotentialImpact,
        risk:PotentialRisk ;
    dct:created "2024-09-30"^^xsd:date ;
    rdfs:isDefinedBy risk: ;
    sw:term_status "accepted"@en ;
    skos:broader risk:Discrimination ;
    skos:definition "Discrimination based on a person's language, often linked to national origin or ethnicity"@en ;
    skos:inScheme risk:risk-taxonomy-classes ;
    skos:prefLabel "Language Discrimination"@en .

risk:LegalComplianceRisk a rdfs:Class,
        skos:Concept,
        dpv:RiskConcept,
        risk:PotentialConsequence,
        risk:PotentialRisk,
        risk:PotentialRiskSource ;
    dct:created "2024-12-17"^^xsd:date ;
    rdfs:isDefinedBy risk: ;
    sw:term_status "accepted"@en ;
    skos:broader risk:LegalRiskConcept ;
    skos:definition "Risks and consequences regarding legal compliance and its violation"@en ;
    skos:inScheme risk:risk-taxonomy-classes ;
    skos:prefLabel "Legal Compliance Risk"@en .

risk:LegalRiskConcept a rdfs:Class,
        skos:Concept,
        dpv:RiskConcept,
        risk:PotentialConsequence,
        risk:PotentialImpact,
        risk:PotentialRisk,
        risk:PotentialRiskSource ;
    dct:created "2024-10-21"^^xsd:date ;
    rdfs:isDefinedBy risk: ;
    sw:term_status "accepted"@en ;
    skos:broader dpv:RiskConcept ;
    skos:definition "Risk concepts, including any potential risk sources, consequences, or impacts, that are legal in nature or relate to a legal system or process"@en ;
    skos:inScheme risk:risk-taxonomy-classes ;
    skos:prefLabel "Legal Risk Concept"@en ;
    skos:scopeNote "Legal in this context refers exclusively to the law applied within a jurisdiction and does not include internal policies or rules within an organisation"@en .

risk:LegalSupportLimited a rdfs:Class,
        skos:Concept,
        dpv:RiskConcept,
        risk:PotentialConsequence,
        risk:PotentialImpact,
        risk:PotentialRisk ;
    dct:created "2024-10-21"^^xsd:date ;
    rdfs:isDefinedBy risk: ;
    sw:term_status "accepted"@en ;
    skos:broader risk:ServiceRelatedConsequence ;
    skos:definition "Concept representing limitation of legal support"@en ;
    skos:inScheme risk:risk-taxonomy-classes ;
    skos:prefLabel "Legal Support Limited"@en .

risk:LegallyRelevantConsequence a rdfs:Class,
        skos:Concept,
        dpv:RiskConcept,
        risk:PotentialConsequence,
        risk:PotentialImpact,
        risk:PotentialRisk ;
    dct:created "2024-12-17"^^xsd:date ;
    rdfs:isDefinedBy risk: ;
    sw:term_status "accepted"@en ;
    skos:broader risk:LegalRiskConcept ;
    skos:definition "A consequence that is legally relevant i.e. actionable under law"@en ;
    skos:inScheme risk:risk-taxonomy-classes ;
    skos:prefLabel "Legally Relevant Consequence"@en .

risk:LoggingControl a rdfs:Class,
        skos:Concept,
        risk:RiskControl ;
    dct:contributor _:person-delaram-golpayegani,
        _:person-harshvardhan-j-pandit ;
    dct:created "2025-01-06"^^xsd:date ;
    rdfs:isDefinedBy risk: ;
    sw:term_status "accepted"@en ;
    skos:broader risk:MonitorControl ;
    skos:definition "Control that logs an event"@en ;
    skos:inScheme risk:risk-controls-classes ;
    skos:prefLabel "Logging Control"@en ;
    skos:scopeNote "Log refers to a record of information regarding the event, including whether it has occurred, was prevented from occurring, and any actions or processes taken in response to it or resulting from it"@en .

risk:LowLikelihood a rdfs:Class,
        skos:Concept,
        dpv:Likelihood ;
    dct:contributor _:person-harshvardhan-j-pandit ;
    dct:created "2022-08-18"^^xsd:date ;
    rdf:value 0.25 ;
    rdfs:isDefinedBy risk: ;
    sw:term_status "accepted"@en ;
    skos:broader risk:3LikelihoodLevels,
        risk:5LikelihoodLevels,
        risk:7LikelihoodLevels ;
    skos:definition "Level where Likelihood is Low"@en ;
    skos:inScheme risk:risk-levels-classes ;
    skos:prefLabel "Low Likelihood"@en ;
    skos:scopeNote "The suggested quantitative value for this concept is 0.25 on a scale of 0 to 1"@en .

risk:LowRisk a rdfs:Class,
        skos:Concept,
        dpv:RiskLevel ;
    dct:contributor _:person-harshvardhan-j-pandit ;
    dct:created "2022-08-18"^^xsd:date ;
    rdf:value 0.25 ;
    rdfs:isDefinedBy risk: ;
    sw:term_status "accepted"@en ;
    skos:broader risk:3RiskLevels,
        risk:5RiskLevels,
        risk:7RiskLevels ;
    skos:definition "Level where Risk is Low"@en ;
    skos:inScheme risk:risk-levels-classes ;
    skos:prefLabel "Low Risk"@en ;
    skos:scopeNote "The suggested quantitative value for this concept is 0.25 on a scale of 0 to 1"@en .

risk:LowSeverity a rdfs:Class,
        skos:Concept,
        dpv:Severity ;
    dct:contributor _:person-harshvardhan-j-pandit ;
    dct:created "2022-08-18"^^xsd:date ;
    rdf:value 0.25 ;
    rdfs:isDefinedBy risk: ;
    sw:term_status "accepted"@en ;
    skos:broader risk:3SeverityLevels,
        risk:5SeverityLevels,
        risk:7SeverityLevels ;
    skos:definition "Level where Severity is Low"@en ;
    skos:inScheme risk:risk-levels-classes ;
    skos:prefLabel "Low Severity"@en ;
    skos:scopeNote "The suggested quantitative value for this concept is 0.25 on a scale of 0 to 1"@en .

risk:LoyaltyProgramExclusion a rdfs:Class,
        skos:Concept,
        dpv:RiskConcept,
        risk:PotentialConsequence,
        risk:PotentialImpact,
        risk:PotentialRisk ;
    dct:created "2024-10-21"^^xsd:date ;
    rdfs:isDefinedBy risk: ;
    sw:term_status "accepted"@en ;
    skos:broader risk:ServiceRelatedConsequence ;
    skos:definition "Concept representing exclusion from loyalty program"@en ;
    skos:inScheme risk:risk-taxonomy-classes ;
    skos:prefLabel "Loyalty Program Exclusion"@en .

risk:MaliciousActivity a rdfs:Class,
        skos:Concept,
        dpv:RiskConcept,
        risk:PotentialConsequence,
        risk:PotentialRisk,
        risk:PotentialRiskSource ;
    dct:created "2024-12-17"^^xsd:date ;
    rdfs:isDefinedBy risk: ;
    sw:term_status "accepted"@en ;
    skos:broader risk:ExternalSecurityThreat ;
    skos:definition "Intentional actions designed to harm, exploit, manipulate, or disrupt individuals, systems, or organizations for personal gain or detriment to others"@en ;
    skos:inScheme risk:risk-taxonomy-classes ;
    skos:prefLabel "Malicious Activity"@en .

risk:MaliciousCodeAttack a rdfs:Class,
        skos:Concept,
        dpv:RiskConcept,
        risk:AvailabilityConcept,
        risk:ConfidentialityConcept,
        risk:IntegrityConcept,
        risk:PotentialRisk,
        risk:PotentialRiskSource ;
    dct:contributor _:person-harshvardhan-j-pandit ;
    dct:created "2022-08-17"^^xsd:date ;
    dct:modified "2024-08-16"^^xsd:date ;
    dct:source _:b7191aa21b975cb14bbce32aa3ba9c7eb ;
    rdfs:isDefinedBy risk: ;
    sw:term_status "accepted"@en ;
    skos:broader risk:SecurityAttack ;
    skos:definition "Concept representing Malicious Code Attack"@en ;
    skos:inScheme risk:risk-taxonomy-classes ;
    skos:prefLabel "Malicious Code Attack"@en .

risk:MalwareAttack a rdfs:Class,
        skos:Concept,
        dpv:RiskConcept,
        risk:AvailabilityConcept,
        risk:ConfidentialityConcept,
        risk:IntegrityConcept,
        risk:PotentialRisk,
        risk:PotentialRiskSource ;
    dct:contributor _:person-harshvardhan-j-pandit ;
    dct:created "2022-08-17"^^xsd:date ;
    dct:modified "2024-08-16"^^xsd:date ;
    dct:source _:bba19dc259a53f0cb59375372938fbb0a ;
    rdfs:isDefinedBy risk: ;
    sw:term_status "accepted"@en ;
    skos:broader risk:SecurityAttack ;
    skos:definition "Concept representing Malware Attack"@en ;
    skos:inScheme risk:risk-taxonomy-classes ;
    skos:prefLabel "Malware Attack"@en .

risk:MaterialDamage a rdfs:Class,
        skos:Concept,
        dpv:RiskConcept,
        risk:PotentialConsequence,
        risk:PotentialImpact,
        risk:PotentialRisk ;
    dct:contributor _:person-harshvardhan-j-pandit ;
    dct:created "2022-03-30"^^xsd:date ;
    dct:modified "2024-08-16"^^xsd:date ;
    rdfs:isDefinedBy risk: ;
    sw:term_status "accepted"@en ;
    skos:broader risk:LegallyRelevantConsequence ;
    skos:definition "Concept representing Material Damage"@en ;
    skos:inScheme risk:risk-taxonomy-classes ;
    skos:prefLabel "Material Damage"@en ;
    skos:scopeNote "The criteria for what is considered material damage is based in jurisdictional laws and norms"@en .

risk:MentalHealth a rdfs:Class,
        skos:Concept,
        dpv:RiskConcept,
        risk:PotentialConsequence,
        risk:PotentialImpact,
        risk:PotentialRisk ;
    dct:contributor _:person-harshvardhan-j-pandit ;
    dct:created "2024-12-01"^^xsd:date ;
    rdfs:isDefinedBy risk: ;
    sw:term_status "accepted"@en ;
    skos:broader risk:Health ;
    skos:definition "Concept representing mental health of individual(s), or group(s), or society at large"@en ;
    skos:inScheme risk:risk-taxonomy-classes ;
    skos:prefLabel "Mental Health"@en .

risk:MentalSafety a rdfs:Class,
        skos:Concept,
        dpv:RiskConcept,
        risk:PotentialConsequence,
        risk:PotentialImpact,
        risk:PotentialRisk ;
    dct:contributor _:person-harshvardhan-j-pandit ;
    dct:created "2024-12-01"^^xsd:date ;
    rdfs:isDefinedBy risk: ;
    sw:term_status "accepted"@en ;
    skos:broader risk:Safety ;
    skos:definition "Concept representing mental safety of individual(s), or group(s), or society at large"@en ;
    skos:inScheme risk:risk-taxonomy-classes ;
    skos:prefLabel "Mental Safety"@en .

risk:Misandry a rdfs:Class,
        skos:Concept,
        dpv:RiskConcept,
        risk:PotentialConsequence,
        risk:PotentialImpact,
        risk:PotentialRisk ;
    dct:created "2024-09-30"^^xsd:date ;
    rdfs:isDefinedBy risk: ;
    sw:term_status "accepted"@en ;
    skos:broader risk:Sexism ;
    skos:definition "Dislike, contempt, or prejudice against men"@en ;
    skos:inScheme risk:risk-taxonomy-classes ;
    skos:prefLabel "Misandry"@en .

risk:Misogyny a rdfs:Class,
        skos:Concept,
        dpv:RiskConcept,
        risk:PotentialConsequence,
        risk:PotentialImpact,
        risk:PotentialRisk ;
    dct:created "2024-09-30"^^xsd:date ;
    rdfs:isDefinedBy risk: ;
    sw:term_status "accepted"@en ;
    skos:broader risk:Sexism ;
    skos:definition "Dislike, contempt, or prejudice against women"@en ;
    skos:inScheme risk:risk-taxonomy-classes ;
    skos:prefLabel "Misogyny"@en .

risk:Misuse a rdfs:Class,
        skos:Concept,
        dpv:RiskConcept,
        risk:PotentialConsequence,
        risk:PotentialRisk,
        risk:PotentialRiskSource ;
    dct:contributor _:person-delaram-golpayegani ;
    dct:created "2024-06-11"^^xsd:date ;
    dct:modified "2024-08-16"^^xsd:date ;
    rdfs:isDefinedBy risk: ;
    sw:term_status "accepted"@en ;
    skos:broader risk:UserRisks ;
    skos:definition "Concept representing a misuse (of something)"@en ;
    skos:inScheme risk:risk-taxonomy-classes ;
    skos:prefLabel "Misuse"@en .

risk:MitigationControl a rdfs:Class,
        skos:Concept,
        risk:RiskControl ;
    dct:contributor _:person-delaram-golpayegani,
        _:person-harshvardhan-j-pandit ;
    dct:created "2025-01-06"^^xsd:date ;
    rdfs:isDefinedBy risk: ;
    sw:term_status "accepted"@en ;
    skos:broader risk:ProactiveControl ;
    skos:definition "Control that aims to reduce the likelihood or effect of an event with the goal of managing an event accepted to occur"@en ;
    skos:inScheme risk:risk-controls-classes ;
    skos:prefLabel "Mitigation Control"@en ;
    skos:scopeNote "Mitigation requires accepting that an event will occur, and thereby focusing on managing it by reducing its likelihood or effects by adding additional processes to specifically address the event or its effects"@en .

risk:ModerateLikelihood a rdfs:Class,
        skos:Concept,
        dpv:Likelihood ;
    dct:contributor _:person-harshvardhan-j-pandit ;
    dct:created "2022-08-18"^^xsd:date ;
    rdf:value 0.5 ;
    rdfs:isDefinedBy risk: ;
    sw:term_status "accepted"@en ;
    skos:broader risk:3LikelihoodLevels,
        risk:5LikelihoodLevels,
        risk:7LikelihoodLevels ;
    skos:definition "Level where Likelihood is Moderate"@en ;
    skos:inScheme risk:risk-levels-classes ;
    skos:prefLabel "Moderate Likelihood"@en ;
    skos:scopeNote "The suggested quantitative value for this concept is 0.5 on a scale of 0 to 1"@en .

risk:ModerateRisk a rdfs:Class,
        skos:Concept,
        dpv:RiskLevel ;
    dct:contributor _:person-harshvardhan-j-pandit ;
    dct:created "2022-08-18"^^xsd:date ;
    rdf:value 0.5 ;
    rdfs:isDefinedBy risk: ;
    sw:term_status "accepted"@en ;
    skos:broader risk:3RiskLevels,
        risk:5RiskLevels,
        risk:7RiskLevels ;
    skos:definition "Level where Risk is Moderate"@en ;
    skos:inScheme risk:risk-levels-classes ;
    skos:prefLabel "Moderate Risk"@en ;
    skos:scopeNote "The suggested quantitative value for this concept is 0.5 on a scale of 0 to 1"@en .

risk:ModerateSeverity a rdfs:Class,
        skos:Concept,
        dpv:Severity ;
    dct:contributor _:person-harshvardhan-j-pandit ;
    dct:created "2022-08-18"^^xsd:date ;
    rdf:value 0.5 ;
    rdfs:isDefinedBy risk: ;
    sw:term_status "accepted"@en ;
    skos:broader risk:3SeverityLevels,
        risk:5SeverityLevels,
        risk:7SeverityLevels ;
    skos:definition "Level where Severity is Moderate"@en ;
    skos:inScheme risk:risk-levels-classes ;
    skos:prefLabel "Moderate Severity"@en ;
    skos:scopeNote "The suggested quantitative value for this concept is 0.5 on a scale of 0 to 1"@en .

risk:ModificationControl a rdfs:Class,
        skos:Concept,
        risk:RiskControl ;
    dct:contributor _:person-delaram-golpayegani,
        _:person-harshvardhan-j-pandit ;
    dct:created "2025-01-06"^^xsd:date ;
    rdfs:isDefinedBy risk: ;
    sw:term_status "accepted"@en ;
    skos:broader risk:ProactiveControl ;
    skos:definition "Control that modifies the context to change the event's characteristics such that the event still occurs but with the modified characteristics with the goal of managing an event that is accepted to occur"@en ;
    skos:inScheme risk:risk-controls-classes ;
    skos:prefLabel "Modification Control"@en ;
    skos:scopeNote "Modification necessitates a change in the context to result in a change in the event's characteristics. Where such changes reduce the likelihood or effects of the event, the modification also works as a mitigation for the event"@en .

risk:MonitorConsequence a rdfs:Class,
        skos:Concept,
        risk:RiskControl ;
    dct:contributor _:person-harshvardhan-j-pandit ;
    dct:created "2024-05-19"^^xsd:date ;
    dct:modified "2025-01-06"^^xsd:date ;
    rdfs:isDefinedBy risk: ;
    sw:term_status "modified"@en ;
    skos:broader risk:MonitorControl ;
    skos:definition "Control that monitors a Risk Consequence"@en ;
    skos:inScheme risk:risk-controls-classes ;
    skos:prefLabel "Monitor Consequence"@en .

risk:MonitorControl a rdfs:Class,
        skos:Concept,
        risk:RiskControl ;
    dct:contributor _:person-harshvardhan-j-pandit ;
    dct:created "2024-05-19"^^xsd:date ;
    dct:modified "2025-01-06"^^xsd:date ;
    rdfs:isDefinedBy risk: ;
    sw:term_status "modified"@en ;
    skos:broader risk:ProactiveControl ;
    skos:definition "Control that monitors for the occurrence of an event"@en ;
    skos:inScheme risk:risk-controls-classes ;
    skos:prefLabel "Monitor Control"@en ;
    skos:scopeNote "Monitoring is a broad term that refers to identifying information about an event, including its occurrence, characteristics such as severity or specific contextual metrics, affected things and entities, and having the ability to obtain and use this information to address the event. Monitoring is also used to refer to the activities associated with ensuring controls are active and effective. For this reason, specific concepts are defined which extend this control to express explicit actions included in the general use of 'monitoring' in risk management"@en .

risk:MonitorImpact a rdfs:Class,
        skos:Concept,
        risk:RiskControl ;
    dct:contributor _:person-harshvardhan-j-pandit ;
    dct:created "2024-05-19"^^xsd:date ;
    dct:modified "2025-01-06"^^xsd:date ;
    rdfs:isDefinedBy risk: ;
    sw:term_status "modified"@en ;
    skos:broader risk:MonitorControl ;
    skos:definition "Control that monitors a Risk Impact"@en ;
    skos:inScheme risk:risk-controls-classes ;
    skos:prefLabel "Monitor Impact"@en .

risk:MonitorRisk a rdfs:Class,
        skos:Concept,
        risk:RiskControl ;
    dct:contributor _:person-harshvardhan-j-pandit ;
    dct:created "2024-05-19"^^xsd:date ;
    dct:modified "2025-01-06"^^xsd:date ;
    rdfs:isDefinedBy risk: ;
    sw:term_status "modified"@en ;
    skos:broader risk:MonitorControl ;
    skos:definition "Control that monitors a Risk"@en ;
    skos:inScheme risk:risk-controls-classes ;
    skos:prefLabel "Monitor Risk"@en .

risk:MonitorRiskControl a rdfs:Class,
        skos:Concept,
        risk:RiskControl ;
    dct:contributor _:person-harshvardhan-j-pandit ;
    dct:created "2024-05-19"^^xsd:date ;
    dct:modified "2025-01-06"^^xsd:date ;
    rdfs:isDefinedBy risk: ;
    sw:term_status "modified"@en ;
    skos:broader risk:MonitorControl ;
    skos:definition "Control that monitors another Control"@en ;
    skos:inScheme risk:risk-controls-classes ;
    skos:prefLabel "Monitor Control"@en .

risk:MonitorRiskSource a rdfs:Class,
        skos:Concept,
        risk:RiskControl ;
    dct:contributor _:person-harshvardhan-j-pandit ;
    dct:created "2024-05-19"^^xsd:date ;
    dct:modified "2025-01-06"^^xsd:date ;
    rdfs:isDefinedBy risk: ;
    sw:term_status "modified"@en ;
    skos:broader risk:MonitorControl ;
    skos:definition "Control that monitors a Risk Source"@en ;
    skos:inScheme risk:risk-controls-classes ;
    skos:prefLabel "Monitor Risk Source"@en .

risk:MonitorVulnerabilities a rdfs:Class,
        skos:Concept,
        risk:RiskControl ;
    dct:contributor _:person-harshvardhan-j-pandit ;
    dct:created "2024-05-19"^^xsd:date ;
    dct:modified "2025-01-06"^^xsd:date ;
    rdfs:isDefinedBy risk: ;
    sw:term_status "modified"@en ;
    skos:broader risk:MonitorControl ;
    skos:definition "Control that monitors a Risk Vulnerability"@en ;
    skos:inScheme risk:risk-controls-classes ;
    skos:prefLabel "Monitor Vulnerabilities"@en .

risk:NationalityDiscrimination a rdfs:Class,
        skos:Concept,
        dpv:RiskConcept,
        risk:PotentialConsequence,
        risk:PotentialImpact,
        risk:PotentialRisk ;
    dct:created "2024-09-30"^^xsd:date ;
    rdfs:isDefinedBy risk: ;
    sw:term_status "accepted"@en ;
    skos:broader risk:Discrimination ;
    skos:definition "Discrimination based on a person's nationality or citizenship"@en ;
    skos:inScheme risk:risk-taxonomy-classes ;
    skos:prefLabel "Nationality Discrimination"@en .

risk:NegotiatingCapacityLoss a rdfs:Class,
        skos:Concept,
        dpv:RiskConcept,
        risk:PotentialConsequence,
        risk:PotentialImpact,
        risk:PotentialRisk ;
    dct:contributor _:person-harshvardhan-j-pandit ;
    dct:created "2022-08-17"^^xsd:date ;
    dct:modified "2025-08-24"^^xsd:date ;
    dct:source _:b15886bc6e88dcdb258fe59ded7be3abf ;
    rdfs:isDefinedBy risk: ;
    sw:term_status "modified"@en ;
    skos:broader risk:ReputationalRisk ;
    skos:definition "Concept representing Negotiating Capacity Loss"@en ;
    skos:inScheme risk:risk-taxonomy-classes ;
    skos:prefLabel "Negotiating Capacity Loss"@en .

risk:NonMaterialDamage a rdfs:Class,
        skos:Concept,
        dpv:RiskConcept,
        risk:PotentialConsequence,
        risk:PotentialImpact,
        risk:PotentialRisk ;
    dct:contributor _:person-harshvardhan-j-pandit ;
    dct:created "2022-03-30"^^xsd:date ;
    dct:modified "2024-08-16"^^xsd:date ;
    rdfs:isDefinedBy risk: ;
    sw:term_status "accepted"@en ;
    skos:broader risk:LegallyRelevantConsequence ;
    skos:definition "Concept representing Non-Material Damage"@en ;
    skos:inScheme risk:risk-taxonomy-classes ;
    skos:prefLabel "Non-Material Damage"@en ;
    skos:scopeNote "The criteria for what is considered material damage is based in jurisdictional laws and norms"@en .

risk:NonNormalityBias a rdfs:Class,
        skos:Concept,
        dpv:RiskConcept,
        risk:PotentialConsequence,
        risk:PotentialRisk,
        risk:PotentialRiskSource ;
    dct:contributor _:person-daniel-doherty,
        _:person-delaram-golpayegani,
        _:person-harshvardhan-j-pandit ;
    dct:created "2024-09-13"^^xsd:date ;
    dct:source "ISO/IEC 24027:2021"@en ;
    rdfs:isDefinedBy risk: ;
    sw:term_status "accepted"@en ;
    skos:broader risk:StatisticalBias ;
    skos:definition "Bias that occurs when the dataset is subject to a different (i.e. non-normal) distribution (e.g., Chi-Square, Beta, Lorentz, Cauchy, Weibull or Pareto) where the results can be biased and misleading"@en ;
    skos:inScheme risk:risk-taxonomy-classes ;
    skos:prefLabel "Non-Normality Bias"@en .

risk:NonResponseBias a rdfs:Class,
        skos:Concept,
        dpv:RiskConcept,
        risk:PotentialConsequence,
        risk:PotentialRisk,
        risk:PotentialRiskSource ;
    dct:contributor _:person-daniel-doherty,
        _:person-delaram-golpayegani,
        _:person-harshvardhan-j-pandit ;
    dct:created "2024-09-13"^^xsd:date ;
    dct:source "ISO/IEC 24027:2021"@en ;
    rdfs:isDefinedBy risk: ;
    sw:term_status "accepted"@en ;
    skos:broader risk:SelectionBias ;
    skos:definition "Bias that occurs when people from certain groups opt-out of surveys at different rates than users from other groups. This is also called as Participation bias"@en ;
    skos:inScheme risk:risk-taxonomy-classes ;
    skos:prefLabel "Non-Response Bias"@en .

risk:OperationalSecurityRisk a rdfs:Class,
        skos:Concept,
        dpv:RiskConcept,
        risk:PotentialConsequence,
        risk:PotentialRisk,
        risk:PotentialRiskSource ;
    dct:created "2024-12-17"^^xsd:date ;
    rdfs:isDefinedBy risk: ;
    sw:term_status "accepted"@en ;
    skos:broader risk:TechnicalRiskConcept ;
    skos:definition "Risks and issues that arise during operational processes"@en ;
    skos:inScheme risk:risk-taxonomy-classes ;
    skos:prefLabel "Operational Security Risk"@en .

risk:OpportunityLoss a rdfs:Class,
        skos:Concept,
        dpv:RiskConcept,
        risk:PotentialConsequence,
        risk:PotentialImpact,
        risk:PotentialRisk ;
    dct:contributor _:person-harshvardhan-j-pandit ;
    dct:created "2022-08-17"^^xsd:date ;
    dct:modified "2025-08-24"^^xsd:date ;
    dct:source _:b15886bc6e88dcdb258fe59ded7be3abf ;
    rdfs:isDefinedBy risk: ;
    sw:term_status "modified"@en ;
    skos:broader risk:ReputationalRisk ;
    skos:definition "Concept representing Opportunity Loss"@en ;
    skos:inScheme risk:risk-taxonomy-classes ;
    skos:prefLabel "Opportunity Loss"@en .

risk:OrganisationalManagementRisk a rdfs:Class,
        skos:Concept,
        dpv:RiskConcept,
        risk:PotentialConsequence,
        risk:PotentialRisk,
        risk:PotentialRiskSource ;
    dct:contributor _:person-delaram-golpayegani,
        _:person-harshvardhan-j-pandit ;
    dct:created "2024-12-01"^^xsd:date ;
    rdfs:isDefinedBy risk: ;
    sw:term_status "accepted"@en ;
    skos:broader risk:OrganisationalRiskConcept ;
    skos:definition "Concept representing issues and risks associated with the management of operations and resources by the organisation"@en ;
    skos:inScheme risk:risk-taxonomy-classes ;
    skos:prefLabel "Organisational Management Risk"@en .

risk:OrganisationalRiskConcept a rdfs:Class,
        skos:Concept,
        dpv:RiskConcept,
        risk:PotentialConsequence,
        risk:PotentialImpact,
        risk:PotentialRisk,
        risk:PotentialRiskSource ;
    dct:created "2024-10-21"^^xsd:date ;
    rdfs:isDefinedBy risk: ;
    sw:term_status "accepted"@en ;
    skos:broader dpv:RiskConcept ;
    skos:definition "Risk concepts, including any potential risk sources, consequences, or impacts, that are organisational in nature or relate to an organisational process"@en ;
    skos:inScheme risk:risk-taxonomy-classes ;
    skos:prefLabel "Organisational Risk Concept"@en ;
    skos:scopeNote "Organisational in this context refers to an organisation which is not human but is managed by humans"@en .

risk:OutGroupHomogeneityBias a rdfs:Class,
        skos:Concept,
        dpv:RiskConcept,
        risk:PotentialConsequence,
        risk:PotentialRisk,
        risk:PotentialRiskSource ;
    dct:contributor _:person-daniel-doherty,
        _:person-delaram-golpayegani,
        _:person-harshvardhan-j-pandit ;
    dct:created "2024-09-13"^^xsd:date ;
    dct:source "ISO/IEC 24027:2021"@en ;
    rdfs:isDefinedBy risk: ;
    sw:term_status "accepted"@en ;
    skos:broader risk:CognitiveBias ;
    skos:definition "Bias that occurs when seeing out-group members as more alike than in-group members when comparing attitudes, values, personality traits, and other characteristics"@en ;
    skos:inScheme risk:risk-taxonomy-classes ;
    skos:prefLabel "Out-Group Homogeneity Bias"@en .

risk:OverrideControl a rdfs:Class,
        skos:Concept,
        risk:RiskControl ;
    dct:contributor _:person-delaram-golpayegani,
        _:person-harshvardhan-j-pandit ;
    dct:created "2025-01-06"^^xsd:date ;
    rdfs:isDefinedBy risk: ;
    sw:term_status "accepted"@en ;
    skos:broader risk:ReactiveControl ;
    skos:definition "Control that aims to override the event with the goal of avoiding its further effects"@en ;
    skos:inScheme risk:risk-controls-classes ;
    skos:prefLabel "Override Control"@en ;
    skos:scopeNote "Override indicates a (temporary) change or bypassing of usual processes, controls, and measures in response to an event"@en .

risk:OversightControl a rdfs:Class,
        skos:Concept,
        risk:RiskControl ;
    dct:contributor _:person-harshvardhan-j-pandit ;
    dct:created "2025-01-06"^^xsd:date ;
    rdfs:isDefinedBy risk: ;
    sw:term_status "accepted"@en ;
    skos:broader risk:MonitorControl ;
    skos:definition "Control that provides oversight for an event in terms of having information about it and being able to supervise or manage it"@en ;
    skos:inScheme risk:risk-controls-classes ;
    skos:prefLabel "Oversight Control"@en ;
    skos:scopeNote "Oversight can be ambiguously used in terms of having knowledge about an event (see risk:TransparencyControl instead), or being able to identify when it occurs (see risk:DetectionControl instead). The control defined by this concept includes the ability to act on the event as part of the 'oversight' term used in management"@en .

risk:Payment a rdfs:Class,
        skos:Concept,
        dpv:RiskConcept,
        risk:PotentialConsequence,
        risk:PotentialImpact,
        risk:PotentialRisk ;
    dct:contributor _:person-georg-p-krog,
        _:person-harshvardhan-j-pandit ;
    dct:created "2024-04-14"^^xsd:date ;
    dct:modified "2025-08-06"^^xsd:date ;
    rdfs:isDefinedBy risk: ;
    sw:term_status "modified"@en ;
    skos:broader risk:Remuneration ;
    skos:definition "Something that acts as or provides payment e.g. to access a service or purchase resources"@en ;
    skos:inScheme risk:risk-taxonomy-classes ;
    skos:prefLabel "Payment"@en .

risk:PersonalSafetyEndangerment a rdfs:Class,
        skos:Concept,
        dpv:RiskConcept,
        risk:PotentialConsequence,
        risk:PotentialImpact,
        risk:PotentialRisk ;
    dct:contributor _:person-harshvardhan-j-pandit ;
    dct:created "2022-08-17"^^xsd:date ;
    dct:modified "2024-12-01"^^xsd:date ;
    dct:source _:b15886bc6e88dcdb258fe59ded7be3abf ;
    rdfs:isDefinedBy risk: ;
    sw:term_status "modified"@en ;
    skos:broader risk:IndividualRisk ;
    skos:definition "Concept representing Personal Safety Endangerment"@en ;
    skos:inScheme risk:risk-taxonomy-classes ;
    skos:prefLabel "Personal Safety Endangerment"@en .

risk:PersonalisationDisabled a rdfs:Class,
        skos:Concept,
        dpv:RiskConcept,
        risk:PotentialConsequence,
        risk:PotentialImpact,
        risk:PotentialRisk ;
    dct:created "2024-10-21"^^xsd:date ;
    rdfs:isDefinedBy risk: ;
    sw:term_status "accepted"@en ;
    skos:broader risk:ServiceRelatedConsequence ;
    skos:definition "Concept representing personalisation disabled"@en ;
    skos:inScheme risk:risk-taxonomy-classes ;
    skos:prefLabel "Personalisation Disabled"@en .

risk:PersonalisationEnabled a rdfs:Class,
        skos:Concept,
        dpv:RiskConcept,
        risk:PotentialConsequence,
        risk:PotentialImpact,
        risk:PotentialRisk ;
    dct:created "2024-10-21"^^xsd:date ;
    rdfs:isDefinedBy risk: ;
    sw:term_status "accepted"@en ;
    skos:broader risk:ServiceRelatedConsequence ;
    skos:definition "Concept representing personalisation enabled"@en ;
    skos:inScheme risk:risk-taxonomy-classes ;
    skos:prefLabel "Personalisation Enabled"@en .

risk:PhishingScam a rdfs:Class,
        skos:Concept,
        dpv:RiskConcept,
        risk:ConfidentialityConcept,
        risk:PotentialConsequence,
        risk:PotentialRisk,
        risk:PotentialRiskSource ;
    dct:contributor _:person-harshvardhan-j-pandit ;
    dct:created "2022-08-17"^^xsd:date ;
    dct:modified "2026-02-09"^^xsd:date ;
    dct:source _:b89b5ee884952f33d70d4fddc4220b465 ;
    rdfs:isDefinedBy risk: ;
    sw:term_status "modified"@en ;
    skos:broader risk:Scam ;
    skos:definition "Concept representing Phishing Scam"@en ;
    skos:inScheme risk:risk-taxonomy-classes ;
    skos:prefLabel "Phishing Scam"@en .

risk:PhysicalAssault a rdfs:Class,
        skos:Concept,
        dpv:RiskConcept,
        risk:PotentialConsequence,
        risk:PotentialImpact,
        risk:PotentialRisk ;
    dct:contributor _:person-harshvardhan-j-pandit ;
    dct:created "2022-08-17"^^xsd:date ;
    dct:modified "2024-08-16"^^xsd:date ;
    dct:source _:b15886bc6e88dcdb258fe59ded7be3abf ;
    rdfs:isDefinedBy risk: ;
    sw:term_status "accepted"@en ;
    skos:broader risk:Harm,
        risk:PhysicalSafety ;
    skos:definition "Concept representing Physical Assault"@en ;
    skos:inScheme risk:risk-taxonomy-classes ;
    skos:prefLabel "Physical Assault"@en .

risk:PhysicalHarm a rdfs:Class,
        skos:Concept,
        dpv:RiskConcept,
        risk:PotentialConsequence,
        risk:PotentialImpact,
        risk:PotentialRisk ;
    dct:contributor _:person-delaram-golpayegani,
        _:person-harshvardhan-j-pandit ;
    dct:created "2022-08-17"^^xsd:date ;
    dct:modified "2024-12-01"^^xsd:date ;
    rdfs:isDefinedBy risk: ;
    sw:term_status "modified"@en ;
    skos:broader risk:Harm,
        risk:PhysicalHealth ;
    skos:definition "Concept representing physical harm to an individual or individual(s)"@en ;
    skos:inScheme risk:risk-taxonomy-classes ;
    skos:prefLabel "Physical Harm"@en .

risk:PhysicalHealth a rdfs:Class,
        skos:Concept,
        dpv:RiskConcept,
        risk:PotentialConsequence,
        risk:PotentialImpact,
        risk:PotentialRisk ;
    dct:contributor _:person-harshvardhan-j-pandit ;
    dct:created "2024-12-01"^^xsd:date ;
    rdfs:isDefinedBy risk: ;
    sw:term_status "accepted"@en ;
    skos:broader risk:Health ;
    skos:definition "Concept representing physical health of individual(s), or group(s), or society at large"@en ;
    skos:inScheme risk:risk-taxonomy-classes ;
    skos:prefLabel "Physical Health"@en .

risk:PhysicalSafety a rdfs:Class,
        skos:Concept,
        dpv:RiskConcept,
        risk:PotentialConsequence,
        risk:PotentialImpact,
        risk:PotentialRisk ;
    dct:contributor _:person-harshvardhan-j-pandit ;
    dct:created "2024-12-01"^^xsd:date ;
    rdfs:isDefinedBy risk: ;
    sw:term_status "accepted"@en ;
    skos:broader risk:Safety ;
    skos:definition "Concept representing physical safety of individual(s), or group(s), or society at large"@en ;
    skos:inScheme risk:risk-taxonomy-classes ;
    skos:prefLabel "Physical Safety"@en .

risk:PolicyRisk a rdfs:Class,
        skos:Concept,
        dpv:RiskConcept,
        risk:PotentialConsequence,
        risk:PotentialRisk,
        risk:PotentialRiskSource ;
    dct:created "2024-12-17"^^xsd:date ;
    rdfs:isDefinedBy risk: ;
    sw:term_status "accepted"@en ;
    skos:broader risk:LegalRiskConcept ;
    skos:definition "Risks and consequences regarding policy and its associated processes"@en ;
    skos:inScheme risk:risk-taxonomy-classes ;
    skos:prefLabel "Policy Risk"@en .

risk:PotentialConsequence a rdfs:Class,
        skos:Concept ;
    dct:contributor _:person-harshvardhan-j-pandit ;
    dct:created "2024-09-29"^^xsd:date ;
    vann:example dex:E0087 ;
    rdfs:isDefinedBy risk: ;
    rdfs:subClassOf dpv:RiskConcept ;
    sw:term_status "accepted"@en ;
    skos:broader dpv:RiskConcept ;
    skos:definition "Indicates a concept can potentially be a 'consequence concept within an use-case"@en ;
    skos:inScheme risk:risk-taxonomy-classes ;
    skos:prefLabel "Potential Consequence"@en ;
    skos:scopeNote "PotentialConsequence is a suggestion that the concept can be a 'risk' within an use-case - this suggestion is not exclusive and the concept may also be instances of other potential concepts to indicate the multiple possible roles a concept can take. This suggestion can be ignored if it is not applicable to the use-case"@en .

risk:PotentialImpact a rdfs:Class,
        skos:Concept ;
    dct:contributor _:person-harshvardhan-j-pandit ;
    dct:created "2024-09-29"^^xsd:date ;
    vann:example dex:E0087 ;
    rdfs:isDefinedBy risk: ;
    rdfs:subClassOf dpv:RiskConcept ;
    sw:term_status "accepted"@en ;
    skos:broader dpv:RiskConcept ;
    skos:definition "Indicates a concept can potentially be a 'impact' concept within an use-case"@en ;
    skos:inScheme risk:risk-taxonomy-classes ;
    skos:prefLabel "Potential Impact"@en ;
    skos:scopeNote "PotentialImpact is a suggestion that the concept can be a 'risk' within an use-case - this suggestion is not exclusive and the concept may also be instances of other potential concepts to indicate the multiple possible roles a concept can take. This suggestion can be ignored if it is not applicable to the use-case"@en .

risk:PotentialRisk a rdfs:Class,
        skos:Concept ;
    dct:contributor _:person-harshvardhan-j-pandit ;
    dct:created "2024-09-29"^^xsd:date ;
    vann:example dex:E0087 ;
    rdfs:isDefinedBy risk: ;
    rdfs:subClassOf dpv:RiskConcept ;
    sw:term_status "accepted"@en ;
    skos:broader dpv:RiskConcept ;
    skos:definition "Indicates a concept can potentially be a 'risk' concept within an use-case"@en ;
    skos:inScheme risk:risk-taxonomy-classes ;
    skos:prefLabel "Potential Risk"@en ;
    skos:scopeNote "PotentialRisk is a suggestion that the concept can be a 'risk' within an use-case - this suggestion is not exclusive and the concept may also be instances of other potential concepts to indicate the multiple possible roles a concept can take. This suggestion can be ignored if it is not applicable to the use-case"@en .

risk:PotentialRiskSource a rdfs:Class,
        skos:Concept ;
    dct:contributor _:person-harshvardhan-j-pandit ;
    dct:created "2024-09-29"^^xsd:date ;
    vann:example dex:E0087 ;
    rdfs:isDefinedBy risk: ;
    rdfs:subClassOf dpv:RiskConcept ;
    sw:term_status "accepted"@en ;
    skos:broader dpv:RiskConcept ;
    skos:definition "Indicates a concept can potentially be a 'risk source' concept within an use-case"@en ;
    skos:inScheme risk:risk-taxonomy-classes ;
    skos:prefLabel "Potential RiskSource"@en ;
    skos:scopeNote "PotentialRiskSource is a suggestion that the concept can be a 'risk' within an use-case - this suggestion is not exclusive and the concept may also be instances of other potential concepts to indicate the multiple possible roles a concept can take. This suggestion can be ignored if it is not applicable to the use-case"@en .

risk:Privacy a rdfs:Class,
        skos:Concept,
        dpv:RiskConcept,
        risk:PotentialConsequence,
        risk:PotentialImpact,
        risk:PotentialRisk ;
    dct:created "2024-12-17"^^xsd:date ;
    rdfs:isDefinedBy risk: ;
    sw:term_status "accepted"@en ;
    skos:broader risk:IndividualRisk ;
    skos:definition "Concept representing privacy of humans at an individual, group, or larger societal levels"@en ;
    skos:inScheme risk:risk-taxonomy-classes ;
    skos:prefLabel "Privacy"@en .

risk:ProactiveControl a rdfs:Class,
        skos:Concept,
        risk:RiskControl ;
    dct:contributor _:person-harshvardhan-j-pandit ;
    dct:created "2025-01-06"^^xsd:date ;
    rdfs:isDefinedBy risk: ;
    sw:term_status "accepted"@en ;
    skos:broader risk:RiskControl ;
    skos:definition "Control that is established or functions before an event occurs"@en ;
    skos:inScheme risk:risk-controls-classes ;
    skos:prefLabel "Proactive Control"@en ;
    skos:scopeNote "The use of 'proactive' here refers to this control being established to address events before they occur. It does not indicate putting in place controls before the event such as planning ahead for potential use of controls to respond to an incident"@en .

risk:PsychologicalHarm a rdfs:Class,
        skos:Concept,
        dpv:RiskConcept,
        risk:PotentialConsequence,
        risk:PotentialImpact,
        risk:PotentialRisk ;
    dct:contributor _:person-harshvardhan-j-pandit ;
    dct:created "2022-08-17"^^xsd:date ;
    dct:modified "2024-08-16"^^xsd:date ;
    dct:source _:b7191aa21b975cb14bbce32aa3ba9c7eb ;
    rdfs:isDefinedBy risk: ;
    sw:term_status "accepted"@en ;
    skos:broader risk:Harm,
        risk:MentalSafety,
        risk:Wellbeing ;
    skos:definition "Concept representing Psychological Harm"@en ;
    skos:inScheme risk:risk-taxonomy-classes ;
    skos:prefLabel "Psychological Harm"@en .

risk:PublicHealthSafety a rdfs:Class,
        skos:Concept,
        dpv:RiskConcept,
        risk:PotentialConsequence,
        risk:PotentialImpact,
        risk:PotentialRisk ;
    dct:created "2024-12-01"^^xsd:date ;
    rdfs:isDefinedBy risk: ;
    sw:term_status "accepted"@en ;
    skos:broader risk:HealthSafety ;
    skos:definition "Concept representing health and safety of the public at large"@en ;
    skos:inScheme risk:risk-taxonomy-classes ;
    skos:prefLabel "Public Health & Safety"@en .

risk:PublicOrderBreach a rdfs:Class,
        skos:Concept,
        dpv:RiskConcept,
        risk:PotentialConsequence,
        risk:PotentialRisk ;
    dct:contributor _:person-harshvardhan-j-pandit ;
    dct:created "2022-08-17"^^xsd:date ;
    dct:modified "2024-08-16"^^xsd:date ;
    dct:source _:b15886bc6e88dcdb258fe59ded7be3abf ;
    rdfs:isDefinedBy risk: ;
    sw:term_status "accepted"@en ;
    skos:broader risk:LegalComplianceRisk ;
    skos:definition "Concept representing Public Order Breach"@en ;
    skos:inScheme risk:risk-taxonomy-classes ;
    skos:prefLabel "Public Order Breach"@en .

risk:PublicServicesExclusion a rdfs:Class,
        skos:Concept,
        dpv:RiskConcept,
        risk:PotentialConsequence,
        risk:PotentialImpact,
        risk:PotentialRisk ;
    dct:created "2024-10-21"^^xsd:date ;
    rdfs:isDefinedBy risk: ;
    sw:term_status "accepted"@en ;
    skos:broader risk:ServiceRelatedConsequence ;
    skos:definition "Concept representing exclusion from public services"@en ;
    skos:inScheme risk:risk-taxonomy-classes ;
    skos:prefLabel "Public Services Exclusion"@en .

risk:QualityDegraded a rdfs:Class,
        skos:Concept,
        dpv:RiskConcept,
        risk:PotentialConsequence,
        risk:PotentialRisk,
        risk:PotentialRiskSource ;
    dct:contributor _:person-harshvardhan-j-pandit ;
    dct:created "2024-12-01"^^xsd:date ;
    rdfs:isDefinedBy risk: ;
    sw:term_status "accepted"@en ;
    skos:broader risk:QualityRisk ;
    skos:definition "Concepts representing risks and issues where Quality is Degraded"@en ;
    skos:inScheme risk:risk-taxonomy-classes ;
    skos:prefLabel "Quality Degraded"@en .

risk:QualityInconsistent a rdfs:Class,
        skos:Concept,
        dpv:RiskConcept,
        risk:PotentialConsequence,
        risk:PotentialRisk,
        risk:PotentialRiskSource ;
    dct:contributor _:person-harshvardhan-j-pandit ;
    dct:created "2024-12-01"^^xsd:date ;
    rdfs:isDefinedBy risk: ;
    sw:term_status "accepted"@en ;
    skos:broader risk:QualityRisk ;
    skos:definition "Concepts representing risks and issues where Quality is Inconsistent"@en ;
    skos:inScheme risk:risk-taxonomy-classes ;
    skos:prefLabel "Quality Inconsistent"@en .

risk:QualityInsufficient a rdfs:Class,
        skos:Concept,
        dpv:RiskConcept,
        risk:PotentialConsequence,
        risk:PotentialRisk,
        risk:PotentialRiskSource ;
    dct:contributor _:person-harshvardhan-j-pandit ;
    dct:created "2024-12-01"^^xsd:date ;
    rdfs:isDefinedBy risk: ;
    sw:term_status "accepted"@en ;
    skos:broader risk:QualityRisk ;
    skos:definition "Concepts representing risks and issues where Quality is Insufficient"@en ;
    skos:inScheme risk:risk-taxonomy-classes ;
    skos:prefLabel "Quality Insufficient"@en .

risk:QualityRisk a rdfs:Class,
        skos:Concept,
        dpv:RiskConcept,
        risk:PotentialConsequence,
        risk:PotentialRisk,
        risk:PotentialRiskSource ;
    dct:contributor _:person-harshvardhan-j-pandit ;
    dct:created "2024-12-01"^^xsd:date ;
    rdfs:isDefinedBy risk: ;
    sw:term_status "accepted"@en ;
    skos:broader risk:OperationalSecurityRisk ;
    skos:definition "Concept representing risks and issues associated with quality of tasks, resources, processes"@en ;
    skos:inScheme risk:risk-taxonomy-classes ;
    skos:prefLabel "Quality Risk"@en .

risk:QualityUnknown a rdfs:Class,
        skos:Concept,
        dpv:RiskConcept,
        risk:PotentialConsequence,
        risk:PotentialRisk,
        risk:PotentialRiskSource ;
    dct:contributor _:person-harshvardhan-j-pandit ;
    dct:created "2024-12-01"^^xsd:date ;
    rdfs:isDefinedBy risk: ;
    sw:term_status "accepted"@en ;
    skos:broader risk:QualityRisk ;
    skos:definition "Concepts representing risks and issues where Quality is Unknown"@en ;
    skos:inScheme risk:risk-taxonomy-classes ;
    skos:prefLabel "Quality Unknown"@en .

risk:QualityUnverified a rdfs:Class,
        skos:Concept,
        dpv:RiskConcept,
        risk:PotentialConsequence,
        risk:PotentialRisk,
        risk:PotentialRiskSource ;
    dct:contributor _:person-harshvardhan-j-pandit ;
    dct:created "2024-12-01"^^xsd:date ;
    rdfs:isDefinedBy risk: ;
    sw:term_status "accepted"@en ;
    skos:broader risk:QualityRisk ;
    skos:definition "Concepts representing risks and issues where Quality is Unverified"@en ;
    skos:inScheme risk:risk-taxonomy-classes ;
    skos:prefLabel "Quality Unverified"@en .

risk:RM3x3S1L1 a rdfs:Class,
        skos:Concept,
        risk:RiskAnalysis ;
    dct:contributor _:person-harshvardhan-j-pandit ;
    dct:created "2022-08-17"^^xsd:date ;
    rdf:value 0.11 ;
    rdfs:isDefinedBy risk: ;
    sw:term_status "accepted"@en ;
    skos:broader risk:RiskMatrix3x3 ;
    skos:definition "Node in a 3x3 Risk Matrix with Risk Severity: Low; Likelihood: Low; and Risk Level: Low"@en ;
    skos:inScheme risk:risk-matrix-classes ;
    skos:prefLabel "Low Risk (RM3x3 S:1 L:1)"@en ;
    dpv:hasLikelihood risk:LowLikelihood ;
    dpv:hasRiskLevel risk:LowRisk ;
    dpv:hasSeverity risk:LowSeverity .

risk:RM3x3S1L2 a rdfs:Class,
        skos:Concept,
        risk:RiskAnalysis ;
    dct:contributor _:person-harshvardhan-j-pandit ;
    dct:created "2022-08-17"^^xsd:date ;
    rdf:value 0.22 ;
    rdfs:isDefinedBy risk: ;
    sw:term_status "accepted"@en ;
    skos:broader risk:RiskMatrix3x3 ;
    skos:definition "Node in a 3x3 Risk Matrix with Risk Severity: Low; Likelihood: Moderate; and Risk Level: Low"@en ;
    skos:inScheme risk:risk-matrix-classes ;
    skos:prefLabel "Low Risk (RM3x3 S:1 L:2)"@en ;
    dpv:hasLikelihood risk:ModerateLikelihood ;
    dpv:hasRiskLevel risk:LowRisk ;
    dpv:hasSeverity risk:LowSeverity .

risk:RM3x3S1L3 a rdfs:Class,
        skos:Concept,
        risk:RiskAnalysis ;
    dct:contributor _:person-harshvardhan-j-pandit ;
    dct:created "2022-08-17"^^xsd:date ;
    rdf:value 0.33 ;
    rdfs:isDefinedBy risk: ;
    sw:term_status "accepted"@en ;
    skos:broader risk:RiskMatrix3x3 ;
    skos:definition "Node in a 3x3 Risk Matrix with Risk Severity: Low; Likelihood: High; and Risk Level: Moderate"@en ;
    skos:inScheme risk:risk-matrix-classes ;
    skos:prefLabel "Moderate Risk (RM3x3 S:1 L:3)"@en ;
    dpv:hasLikelihood risk:HighLikelihood ;
    dpv:hasRiskLevel risk:ModerateRisk ;
    dpv:hasSeverity risk:LowSeverity .

risk:RM3x3S2L1 a rdfs:Class,
        skos:Concept,
        risk:RiskAnalysis ;
    dct:contributor _:person-harshvardhan-j-pandit ;
    dct:created "2022-08-17"^^xsd:date ;
    rdf:value 0.22 ;
    rdfs:isDefinedBy risk: ;
    sw:term_status "accepted"@en ;
    skos:broader risk:RiskMatrix3x3 ;
    skos:definition "Node in a 3x3 Risk Matrix with Risk Severity: Moderate; Likelihood: Low; and Risk Level: Low"@en ;
    skos:inScheme risk:risk-matrix-classes ;
    skos:prefLabel "Low Risk (RM3x3 S:2 L:1)"@en ;
    dpv:hasLikelihood risk:LowLikelihood ;
    dpv:hasRiskLevel risk:LowRisk ;
    dpv:hasSeverity risk:ModerateSeverity .

risk:RM3x3S2L2 a rdfs:Class,
        skos:Concept,
        risk:RiskAnalysis ;
    dct:contributor _:person-harshvardhan-j-pandit ;
    dct:created "2022-08-17"^^xsd:date ;
    rdf:value 0.44 ;
    rdfs:isDefinedBy risk: ;
    sw:term_status "accepted"@en ;
    skos:broader risk:RiskMatrix3x3 ;
    skos:definition "Node in a 3x3 Risk Matrix with Risk Severity: Moderate; Likelihood: Moderate; and Risk Level: Moderate"@en ;
    skos:inScheme risk:risk-matrix-classes ;
    skos:prefLabel "Moderate Risk (RM3x3 S:2 L:2)"@en ;
    dpv:hasLikelihood risk:ModerateLikelihood ;
    dpv:hasRiskLevel risk:ModerateRisk ;
    dpv:hasSeverity risk:ModerateSeverity .

risk:RM3x3S2L3 a rdfs:Class,
        skos:Concept,
        risk:RiskAnalysis ;
    dct:contributor _:person-harshvardhan-j-pandit ;
    dct:created "2022-08-17"^^xsd:date ;
    rdf:value 0.67 ;
    rdfs:isDefinedBy risk: ;
    sw:term_status "accepted"@en ;
    skos:broader risk:RiskMatrix3x3 ;
    skos:definition "Node in a 3x3 Risk Matrix with Risk Severity: Moderate; Likelihood: High; and Risk Level: High"@en ;
    skos:inScheme risk:risk-matrix-classes ;
    skos:prefLabel "High Risk (RM3x3 S:2 L:3)"@en ;
    dpv:hasLikelihood risk:HighLikelihood ;
    dpv:hasRiskLevel risk:HighRisk ;
    dpv:hasSeverity risk:ModerateSeverity .

risk:RM3x3S3L1 a rdfs:Class,
        skos:Concept,
        risk:RiskAnalysis ;
    dct:contributor _:person-harshvardhan-j-pandit ;
    dct:created "2022-08-17"^^xsd:date ;
    rdf:value 0.33 ;
    rdfs:isDefinedBy risk: ;
    sw:term_status "accepted"@en ;
    skos:broader risk:RiskMatrix3x3 ;
    skos:definition "Node in a 3x3 Risk Matrix with Risk Severity: High; Likelihood: Low; and Risk Level: Moderate"@en ;
    skos:inScheme risk:risk-matrix-classes ;
    skos:prefLabel "Moderate Risk (RM3x3 S:3 L:1)"@en ;
    dpv:hasLikelihood risk:LowLikelihood ;
    dpv:hasRiskLevel risk:ModerateRisk ;
    dpv:hasSeverity risk:HighSeverity .

risk:RM3x3S3L2 a rdfs:Class,
        skos:Concept,
        risk:RiskAnalysis ;
    dct:contributor _:person-harshvardhan-j-pandit ;
    dct:created "2022-08-17"^^xsd:date ;
    rdf:value 0.67 ;
    rdfs:isDefinedBy risk: ;
    sw:term_status "accepted"@en ;
    skos:broader risk:RiskMatrix3x3 ;
    skos:definition "Node in a 3x3 Risk Matrix with Risk Severity: High; Likelihood: Moderate; and Risk Level: High"@en ;
    skos:inScheme risk:risk-matrix-classes ;
    skos:prefLabel "High Risk (RM3x3 S:3 L:2)"@en ;
    dpv:hasLikelihood risk:ModerateLikelihood ;
    dpv:hasRiskLevel risk:HighRisk ;
    dpv:hasSeverity risk:HighSeverity .

risk:RM3x3S3L3 a rdfs:Class,
        skos:Concept,
        risk:RiskAnalysis ;
    dct:contributor _:person-harshvardhan-j-pandit ;
    dct:created "2022-08-17"^^xsd:date ;
    rdf:value 0.99 ;
    rdfs:isDefinedBy risk: ;
    sw:term_status "accepted"@en ;
    skos:broader risk:RiskMatrix3x3 ;
    skos:definition "Node in a 3x3 Risk Matrix with Risk Severity: High; Likelihood: High; and Risk Level: High"@en ;
    skos:inScheme risk:risk-matrix-classes ;
    skos:prefLabel "High Risk (RM3x3 S:3 L:3)"@en ;
    dpv:hasLikelihood risk:HighLikelihood ;
    dpv:hasRiskLevel risk:HighRisk ;
    dpv:hasSeverity risk:HighSeverity .

risk:RM5x5S1L1 a rdfs:Class,
        skos:Concept,
        risk:RiskAnalysis ;
    dct:contributor _:person-harshvardhan-j-pandit ;
    dct:created "2022-08-17"^^xsd:date ;
    rdf:value 0.04 ;
    rdfs:isDefinedBy risk: ;
    sw:term_status "accepted"@en ;
    skos:broader risk:RiskMatrix5x5 ;
    skos:definition "Node in a 5x5 Risk Matrix with Risk Severity: Very Low; Likelihood: Very Low; and Risk Level: Very Low"@en ;
    skos:inScheme risk:risk-matrix-classes ;
    skos:prefLabel "Very Low Risk (RM5x5 S:1 L:1)"@en ;
    dpv:hasLikelihood risk:VeryLowLikelihood ;
    dpv:hasRiskLevel risk:VeryLowRisk ;
    dpv:hasSeverity risk:VeryLowSeverity .

risk:RM5x5S1L2 a rdfs:Class,
        skos:Concept,
        risk:RiskAnalysis ;
    dct:contributor _:person-harshvardhan-j-pandit ;
    dct:created "2022-08-17"^^xsd:date ;
    rdf:value 0.08 ;
    rdfs:isDefinedBy risk: ;
    sw:term_status "accepted"@en ;
    skos:broader risk:RiskMatrix5x5 ;
    skos:definition "Node in a 5x5 Risk Matrix with Risk Severity: Very Low; Likelihood: Low; and Risk Level: Very Low"@en ;
    skos:inScheme risk:risk-matrix-classes ;
    skos:prefLabel "Very Low Risk (RM5x5 S:1 L:2)"@en ;
    dpv:hasLikelihood risk:LowLikelihood ;
    dpv:hasRiskLevel risk:VeryLowRisk ;
    dpv:hasSeverity risk:VeryLowSeverity .

risk:RM5x5S1L3 a rdfs:Class,
        skos:Concept,
        risk:RiskAnalysis ;
    dct:contributor _:person-harshvardhan-j-pandit ;
    dct:created "2022-08-17"^^xsd:date ;
    rdf:value 0.12 ;
    rdfs:isDefinedBy risk: ;
    sw:term_status "accepted"@en ;
    skos:broader risk:RiskMatrix5x5 ;
    skos:definition "Node in a 5x5 Risk Matrix with Risk Severity: Very Low; Likelihood: Moderate; and Risk Level: Very Low"@en ;
    skos:inScheme risk:risk-matrix-classes ;
    skos:prefLabel "Very Low Risk (RM5x5 S:1 L:3)"@en ;
    dpv:hasLikelihood risk:ModerateLikelihood ;
    dpv:hasRiskLevel risk:VeryLowRisk ;
    dpv:hasSeverity risk:VeryLowSeverity .

risk:RM5x5S1L4 a rdfs:Class,
        skos:Concept,
        risk:RiskAnalysis ;
    dct:contributor _:person-harshvardhan-j-pandit ;
    dct:created "2022-08-17"^^xsd:date ;
    rdf:value 0.16 ;
    rdfs:isDefinedBy risk: ;
    sw:term_status "accepted"@en ;
    skos:broader risk:RiskMatrix5x5 ;
    skos:definition "Node in a 5x5 Risk Matrix with Risk Severity: Very Low; Likelihood: High; and Risk Level: Low"@en ;
    skos:inScheme risk:risk-matrix-classes ;
    skos:prefLabel "Low Risk (RM5x5 S:1 L:4)"@en ;
    dpv:hasLikelihood risk:HighLikelihood ;
    dpv:hasRiskLevel risk:LowRisk ;
    dpv:hasSeverity risk:VeryLowSeverity .

risk:RM5x5S1L5 a rdfs:Class,
        skos:Concept,
        risk:RiskAnalysis ;
    dct:contributor _:person-harshvardhan-j-pandit ;
    dct:created "2022-08-17"^^xsd:date ;
    rdf:value 0.20 ;
    rdfs:isDefinedBy risk: ;
    sw:term_status "accepted"@en ;
    skos:broader risk:RiskMatrix5x5 ;
    skos:definition "Node in a 5x5 Risk Matrix with Risk Severity: Very Low; Likelihood: Very High; and Risk Level: Low"@en ;
    skos:inScheme risk:risk-matrix-classes ;
    skos:prefLabel "Low Risk (RM5x5 S:1 L:5)"@en ;
    dpv:hasLikelihood risk:VeryHighLikelihood ;
    dpv:hasRiskLevel risk:LowRisk ;
    dpv:hasSeverity risk:VeryLowSeverity .

risk:RM5x5S2L1 a rdfs:Class,
        skos:Concept,
        risk:RiskAnalysis ;
    dct:contributor _:person-harshvardhan-j-pandit ;
    dct:created "2022-08-17"^^xsd:date ;
    rdf:value 0.08 ;
    rdfs:isDefinedBy risk: ;
    sw:term_status "accepted"@en ;
    skos:broader risk:RiskMatrix5x5 ;
    skos:definition "Node in a 5x5 Risk Matrix with Risk Severity: Low; Likelihood: Very Low; and Risk Level: Very Low"@en ;
    skos:inScheme risk:risk-matrix-classes ;
    skos:prefLabel "Very Low Risk (RM5x5 S:2 L:1)"@en ;
    dpv:hasLikelihood risk:VeryLowLikelihood ;
    dpv:hasRiskLevel risk:VeryLowRisk ;
    dpv:hasSeverity risk:LowSeverity .

risk:RM5x5S2L2 a rdfs:Class,
        skos:Concept,
        risk:RiskAnalysis ;
    dct:contributor _:person-harshvardhan-j-pandit ;
    dct:created "2022-08-17"^^xsd:date ;
    rdf:value 0.16 ;
    rdfs:isDefinedBy risk: ;
    sw:term_status "accepted"@en ;
    skos:broader risk:RiskMatrix5x5 ;
    skos:definition "Node in a 5x5 Risk Matrix with Risk Severity: Low; Likelihood: Low; and Risk Level: Low"@en ;
    skos:inScheme risk:risk-matrix-classes ;
    skos:prefLabel "Low Risk (RM5x5 S:2 L:2)"@en ;
    dpv:hasLikelihood risk:LowLikelihood ;
    dpv:hasRiskLevel risk:LowRisk ;
    dpv:hasSeverity risk:LowSeverity .

risk:RM5x5S2L3 a rdfs:Class,
        skos:Concept,
        risk:RiskAnalysis ;
    dct:contributor _:person-harshvardhan-j-pandit ;
    dct:created "2022-08-17"^^xsd:date ;
    rdf:value 0.24 ;
    rdfs:isDefinedBy risk: ;
    sw:term_status "accepted"@en ;
    skos:broader risk:RiskMatrix5x5 ;
    skos:definition "Node in a 5x5 Risk Matrix with Risk Severity: Low; Likelihood: Moderate; and Risk Level: Moderate"@en ;
    skos:inScheme risk:risk-matrix-classes ;
    skos:prefLabel "Moderate Risk (RM5x5 S:2 L:3)"@en ;
    dpv:hasLikelihood risk:ModerateLikelihood ;
    dpv:hasRiskLevel risk:ModerateRisk ;
    dpv:hasSeverity risk:LowSeverity .

risk:RM5x5S2L4 a rdfs:Class,
        skos:Concept,
        risk:RiskAnalysis ;
    dct:contributor _:person-harshvardhan-j-pandit ;
    dct:created "2022-08-17"^^xsd:date ;
    rdf:value 0.32 ;
    rdfs:isDefinedBy risk: ;
    sw:term_status "accepted"@en ;
    skos:broader risk:RiskMatrix5x5 ;
    skos:definition "Node in a 5x5 Risk Matrix with Risk Severity: Low; Likelihood: High; and Risk Level: Moderate"@en ;
    skos:inScheme risk:risk-matrix-classes ;
    skos:prefLabel "Moderate Risk (RM5x5 S:2 L:4)"@en ;
    dpv:hasLikelihood risk:HighLikelihood ;
    dpv:hasRiskLevel risk:ModerateRisk ;
    dpv:hasSeverity risk:LowSeverity .

risk:RM5x5S2L5 a rdfs:Class,
        skos:Concept,
        risk:RiskAnalysis ;
    dct:contributor _:person-harshvardhan-j-pandit ;
    dct:created "2022-08-17"^^xsd:date ;
    rdf:value 0.40 ;
    rdfs:isDefinedBy risk: ;
    sw:term_status "accepted"@en ;
    skos:broader risk:RiskMatrix5x5 ;
    skos:definition "Node in a 5x5 Risk Matrix with Risk Severity: Low; Likelihood: Very High; and Risk Level: High"@en ;
    skos:inScheme risk:risk-matrix-classes ;
    skos:prefLabel "High Risk (RM5x5 S:2 L:5)"@en ;
    dpv:hasLikelihood risk:VeryHighLikelihood ;
    dpv:hasRiskLevel risk:HighRisk ;
    dpv:hasSeverity risk:LowSeverity .

risk:RM5x5S3L1 a rdfs:Class,
        skos:Concept,
        risk:RiskAnalysis ;
    dct:contributor _:person-harshvardhan-j-pandit ;
    dct:created "2022-08-17"^^xsd:date ;
    rdf:value 0.12 ;
    rdfs:isDefinedBy risk: ;
    sw:term_status "accepted"@en ;
    skos:broader risk:RiskMatrix5x5 ;
    skos:definition "Node in a 5x5 Risk Matrix with Risk Severity: Moderate; Likelihood: Very Low; and Risk Level: Very Low"@en ;
    skos:inScheme risk:risk-matrix-classes ;
    skos:prefLabel "Very Low Risk (RM5x5 S:3 L:1)"@en ;
    dpv:hasLikelihood risk:VeryLowLikelihood ;
    dpv:hasRiskLevel risk:VeryLowRisk ;
    dpv:hasSeverity risk:ModerateSeverity .

risk:RM5x5S3L2 a rdfs:Class,
        skos:Concept,
        risk:RiskAnalysis ;
    dct:contributor _:person-harshvardhan-j-pandit ;
    dct:created "2022-08-17"^^xsd:date ;
    rdf:value 0.24 ;
    rdfs:isDefinedBy risk: ;
    sw:term_status "accepted"@en ;
    skos:broader risk:RiskMatrix5x5 ;
    skos:definition "Node in a 5x5 Risk Matrix with Risk Severity: Moderate; Likelihood: Low; and Risk Level: Moderate"@en ;
    skos:inScheme risk:risk-matrix-classes ;
    skos:prefLabel "Moderate Risk (RM5x5 S:3 L:2)"@en ;
    dpv:hasLikelihood risk:LowLikelihood ;
    dpv:hasRiskLevel risk:ModerateRisk ;
    dpv:hasSeverity risk:ModerateSeverity .

risk:RM5x5S3L3 a rdfs:Class,
        skos:Concept,
        risk:RiskAnalysis ;
    dct:contributor _:person-harshvardhan-j-pandit ;
    dct:created "2022-08-17"^^xsd:date ;
    rdf:value 0.36 ;
    rdfs:isDefinedBy risk: ;
    sw:term_status "accepted"@en ;
    skos:broader risk:RiskMatrix5x5 ;
    skos:definition "Node in a 5x5 Risk Matrix with Risk Severity: Moderate; Likelihood: Moderate; and Risk Level: Moderate"@en ;
    skos:inScheme risk:risk-matrix-classes ;
    skos:prefLabel "Moderate Risk (RM5x5 S:3 L:3)"@en ;
    dpv:hasLikelihood risk:ModerateLikelihood ;
    dpv:hasRiskLevel risk:ModerateRisk ;
    dpv:hasSeverity risk:ModerateSeverity .

risk:RM5x5S3L4 a rdfs:Class,
        skos:Concept,
        risk:RiskAnalysis ;
    dct:contributor _:person-harshvardhan-j-pandit ;
    dct:created "2022-08-17"^^xsd:date ;
    rdf:value 0.48 ;
    rdfs:isDefinedBy risk: ;
    sw:term_status "accepted"@en ;
    skos:broader risk:RiskMatrix5x5 ;
    skos:definition "Node in a 5x5 Risk Matrix with Risk Severity: Moderate; Likelihood: High; and Risk Level: High"@en ;
    skos:inScheme risk:risk-matrix-classes ;
    skos:prefLabel "High Risk (RM5x5 S:3 L:4)"@en ;
    dpv:hasLikelihood risk:HighLikelihood ;
    dpv:hasRiskLevel risk:HighRisk ;
    dpv:hasSeverity risk:ModerateSeverity .

risk:RM5x5S3L5 a rdfs:Class,
        skos:Concept,
        risk:RiskAnalysis ;
    dct:contributor _:person-harshvardhan-j-pandit ;
    dct:created "2022-08-17"^^xsd:date ;
    rdf:value 0.60 ;
    rdfs:isDefinedBy risk: ;
    sw:term_status "accepted"@en ;
    skos:broader risk:RiskMatrix5x5 ;
    skos:definition "Node in a 5x5 Risk Matrix with Risk Severity: Moderate; Likelihood: Very High; and Risk Level: Very High"@en ;
    skos:inScheme risk:risk-matrix-classes ;
    skos:prefLabel "Very High Risk (RM5x5 S:3 L:5)"@en ;
    dpv:hasLikelihood risk:VeryHighLikelihood ;
    dpv:hasRiskLevel risk:VeryHighRisk ;
    dpv:hasSeverity risk:ModerateSeverity .

risk:RM5x5S4L1 a rdfs:Class,
        skos:Concept,
        risk:RiskAnalysis ;
    dct:contributor _:person-harshvardhan-j-pandit ;
    dct:created "2022-08-17"^^xsd:date ;
    rdf:value 0.16 ;
    rdfs:isDefinedBy risk: ;
    sw:term_status "accepted"@en ;
    skos:broader risk:RiskMatrix5x5 ;
    skos:definition "Node in a 5x5 Risk Matrix with Risk Severity: High; Likelihood: Very Low; and Risk Level: Low"@en ;
    skos:inScheme risk:risk-matrix-classes ;
    skos:prefLabel "Low Risk (RM5x5 S:4 L:1)"@en ;
    dpv:hasLikelihood risk:VeryLowLikelihood ;
    dpv:hasRiskLevel risk:LowRisk ;
    dpv:hasSeverity risk:HighSeverity .

risk:RM5x5S4L2 a rdfs:Class,
        skos:Concept,
        risk:RiskAnalysis ;
    dct:contributor _:person-harshvardhan-j-pandit ;
    dct:created "2022-08-17"^^xsd:date ;
    rdf:value 0.32 ;
    rdfs:isDefinedBy risk: ;
    sw:term_status "accepted"@en ;
    skos:broader risk:RiskMatrix5x5 ;
    skos:definition "Node in a 5x5 Risk Matrix with Risk Severity: High; Likelihood: Low; and Risk Level: Moderate"@en ;
    skos:inScheme risk:risk-matrix-classes ;
    skos:prefLabel "Moderate Risk (RM5x5 S:4 L:2)"@en ;
    dpv:hasLikelihood risk:LowLikelihood ;
    dpv:hasRiskLevel risk:ModerateRisk ;
    dpv:hasSeverity risk:HighSeverity .

risk:RM5x5S4L3 a rdfs:Class,
        skos:Concept,
        risk:RiskAnalysis ;
    dct:contributor _:person-harshvardhan-j-pandit ;
    dct:created "2022-08-17"^^xsd:date ;
    rdf:value 0.48 ;
    rdfs:isDefinedBy risk: ;
    sw:term_status "accepted"@en ;
    skos:broader risk:RiskMatrix5x5 ;
    skos:definition "Node in a 5x5 Risk Matrix with Risk Severity: High; Likelihood: Moderate; and Risk Level: High"@en ;
    skos:inScheme risk:risk-matrix-classes ;
    skos:prefLabel "High Risk (RM5x5 S:4 L:3)"@en ;
    dpv:hasLikelihood risk:ModerateLikelihood ;
    dpv:hasRiskLevel risk:HighRisk ;
    dpv:hasSeverity risk:HighSeverity .

risk:RM5x5S4L4 a rdfs:Class,
        skos:Concept,
        risk:RiskAnalysis ;
    dct:contributor _:person-harshvardhan-j-pandit ;
    dct:created "2022-08-17"^^xsd:date ;
    rdf:value 0.64 ;
    rdfs:isDefinedBy risk: ;
    sw:term_status "accepted"@en ;
    skos:broader risk:RiskMatrix5x5 ;
    skos:definition "Node in a 5x5 Risk Matrix with Risk Severity: High; Likelihood: High; and Risk Level: Very High"@en ;
    skos:inScheme risk:risk-matrix-classes ;
    skos:prefLabel "Very High Risk (RM5x5 S:4 L:4)"@en ;
    dpv:hasLikelihood risk:HighLikelihood ;
    dpv:hasRiskLevel risk:VeryHighRisk ;
    dpv:hasSeverity risk:HighSeverity .

risk:RM5x5S4L5 a rdfs:Class,
        skos:Concept,
        risk:RiskAnalysis ;
    dct:contributor _:person-harshvardhan-j-pandit ;
    dct:created "2022-08-17"^^xsd:date ;
    rdf:value 0.80 ;
    rdfs:isDefinedBy risk: ;
    sw:term_status "accepted"@en ;
    skos:broader risk:RiskMatrix5x5 ;
    skos:definition "Node in a 5x5 Risk Matrix with Risk Severity: High; Likelihood: Very High; and Risk Level: Very High"@en ;
    skos:inScheme risk:risk-matrix-classes ;
    skos:prefLabel "Very High Risk (RM5x5 S:4 L:5)"@en ;
    dpv:hasLikelihood risk:VeryHighLikelihood ;
    dpv:hasRiskLevel risk:VeryHighRisk ;
    dpv:hasSeverity risk:HighSeverity .

risk:RM5x5S5L1 a rdfs:Class,
        skos:Concept,
        risk:RiskAnalysis ;
    dct:contributor _:person-harshvardhan-j-pandit ;
    dct:created "2022-08-17"^^xsd:date ;
    rdf:value 0.20 ;
    rdfs:isDefinedBy risk: ;
    sw:term_status "accepted"@en ;
    skos:broader risk:RiskMatrix5x5 ;
    skos:definition "Node in a 5x5 Risk Matrix with Risk Severity: Very High; Likelihood: Very Low; and Risk Level: Low"@en ;
    skos:inScheme risk:risk-matrix-classes ;
    skos:prefLabel "Low Risk (RM5x5 S:5 L:1)"@en ;
    dpv:hasLikelihood risk:VeryLowLikelihood ;
    dpv:hasRiskLevel risk:LowRisk ;
    dpv:hasSeverity risk:VeryHighSeverity .

risk:RM5x5S5L2 a rdfs:Class,
        skos:Concept,
        risk:RiskAnalysis ;
    dct:contributor _:person-harshvardhan-j-pandit ;
    dct:created "2022-08-17"^^xsd:date ;
    rdf:value 0.40 ;
    rdfs:isDefinedBy risk: ;
    sw:term_status "accepted"@en ;
    skos:broader risk:RiskMatrix5x5 ;
    skos:definition "Node in a 5x5 Risk Matrix with Risk Severity: Very High; Likelihood: Low; and Risk Level: High"@en ;
    skos:inScheme risk:risk-matrix-classes ;
    skos:prefLabel "High Risk (RM5x5 S:5 L:2)"@en ;
    dpv:hasLikelihood risk:LowLikelihood ;
    dpv:hasRiskLevel risk:HighRisk ;
    dpv:hasSeverity risk:VeryHighSeverity .

risk:RM5x5S5L3 a rdfs:Class,
        skos:Concept,
        risk:RiskAnalysis ;
    dct:contributor _:person-harshvardhan-j-pandit ;
    dct:created "2022-08-17"^^xsd:date ;
    rdf:value 0.60 ;
    rdfs:isDefinedBy risk: ;
    sw:term_status "accepted"@en ;
    skos:broader risk:RiskMatrix5x5 ;
    skos:definition "Node in a 5x5 Risk Matrix with Risk Severity: Very High; Likelihood: Moderate; and Risk Level: High"@en ;
    skos:inScheme risk:risk-matrix-classes ;
    skos:prefLabel "High Risk (RM5x5 S:5 L:3)"@en ;
    dpv:hasLikelihood risk:ModerateLikelihood ;
    dpv:hasRiskLevel risk:HighRisk ;
    dpv:hasSeverity risk:VeryHighSeverity .

risk:RM5x5S5L4 a rdfs:Class,
        skos:Concept,
        risk:RiskAnalysis ;
    dct:contributor _:person-harshvardhan-j-pandit ;
    dct:created "2022-08-17"^^xsd:date ;
    rdf:value 0.80 ;
    rdfs:isDefinedBy risk: ;
    sw:term_status "accepted"@en ;
    skos:broader risk:RiskMatrix5x5 ;
    skos:definition "Node in a 5x5 Risk Matrix with Risk Severity: Very High; Likelihood: High; and Risk Level: Very High"@en ;
    skos:inScheme risk:risk-matrix-classes ;
    skos:prefLabel "Very High Risk (RM5x5 S:5 L:4)"@en ;
    dpv:hasLikelihood risk:HighLikelihood ;
    dpv:hasRiskLevel risk:VeryHighRisk ;
    dpv:hasSeverity risk:VeryHighSeverity .

risk:RM5x5S5L5 a rdfs:Class,
        skos:Concept,
        risk:RiskAnalysis ;
    dct:contributor _:person-harshvardhan-j-pandit ;
    dct:created "2022-08-17"^^xsd:date ;
    rdf:value 0.99 ;
    rdfs:isDefinedBy risk: ;
    sw:term_status "accepted"@en ;
    skos:broader risk:RiskMatrix5x5 ;
    skos:definition "Node in a 5x5 Risk Matrix with Risk Severity: Very High; Likelihood: Very High; and Risk Level: Very High"@en ;
    skos:inScheme risk:risk-matrix-classes ;
    skos:prefLabel "Very High Risk (RM5x5 S:5 L:5)"@en ;
    dpv:hasLikelihood risk:VeryHighLikelihood ;
    dpv:hasRiskLevel risk:VeryHighRisk ;
    dpv:hasSeverity risk:VeryHighSeverity .

risk:RM7x7S1L1 a rdfs:Class,
        skos:Concept,
        risk:RiskAnalysis ;
    dct:contributor _:person-harshvardhan-j-pandit ;
    dct:created "2022-08-17"^^xsd:date ;
    rdf:value 0.02 ;
    rdfs:isDefinedBy risk: ;
    sw:term_status "accepted"@en ;
    skos:broader risk:RiskMatrix7x7 ;
    skos:definition "Node in a 7x7 Risk Matrix with Risk Severity: Extremely Low; Likelihood: Extremely Low; and Risk Level: Extremely Low"@en ;
    skos:inScheme risk:risk-matrix-classes ;
    skos:prefLabel "Extremely Low Risk (RM7x7 S:1 L:1)"@en ;
    dpv:hasLikelihood risk:ExtremelyLowLikelihood ;
    dpv:hasRiskLevel risk:ExtremelyLowRisk ;
    dpv:hasSeverity risk:ExtremelyLowSeverity .

risk:RM7x7S1L2 a rdfs:Class,
        skos:Concept,
        risk:RiskAnalysis ;
    dct:contributor _:person-harshvardhan-j-pandit ;
    dct:created "2022-08-17"^^xsd:date ;
    rdf:value 0.04 ;
    rdfs:isDefinedBy risk: ;
    sw:term_status "accepted"@en ;
    skos:broader risk:RiskMatrix7x7 ;
    skos:definition "Node in a 7x7 Risk Matrix with Risk Severity: Extremely Low; Likelihood: Very Low; and Risk Level: Extremely Low"@en ;
    skos:inScheme risk:risk-matrix-classes ;
    skos:prefLabel "Extremely Low Risk (RM7x7 S:1 L:2)"@en ;
    dpv:hasLikelihood risk:VeryLowLikelihood ;
    dpv:hasRiskLevel risk:ExtremelyLowRisk ;
    dpv:hasSeverity risk:ExtremelyLowSeverity .

risk:RM7x7S1L3 a rdfs:Class,
        skos:Concept,
        risk:RiskAnalysis ;
    dct:contributor _:person-harshvardhan-j-pandit ;
    dct:created "2022-08-17"^^xsd:date ;
    rdf:value 0.06 ;
    rdfs:isDefinedBy risk: ;
    sw:term_status "accepted"@en ;
    skos:broader risk:RiskMatrix7x7 ;
    skos:definition "Node in a 7x7 Risk Matrix with Risk Severity: Extremely Low; Likelihood: Low; and Risk Level: Extremely Low"@en ;
    skos:inScheme risk:risk-matrix-classes ;
    skos:prefLabel "Extremely Low Risk (RM7x7 S:1 L:3)"@en ;
    dpv:hasLikelihood risk:LowLikelihood ;
    dpv:hasRiskLevel risk:ExtremelyLowRisk ;
    dpv:hasSeverity risk:ExtremelyLowSeverity .

risk:RM7x7S1L4 a rdfs:Class,
        skos:Concept,
        risk:RiskAnalysis ;
    dct:contributor _:person-harshvardhan-j-pandit ;
    dct:created "2022-08-17"^^xsd:date ;
    rdf:value 0.08 ;
    rdfs:isDefinedBy risk: ;
    sw:term_status "accepted"@en ;
    skos:broader risk:RiskMatrix7x7 ;
    skos:definition "Node in a 7x7 Risk Matrix with Risk Severity: Extremely Low; Likelihood: Moderate; and Risk Level: Very Low"@en ;
    skos:inScheme risk:risk-matrix-classes ;
    skos:prefLabel "Very Low Risk (RM7x7 S:1 L:4)"@en ;
    dpv:hasLikelihood risk:ModerateLikelihood ;
    dpv:hasRiskLevel risk:VeryLowRisk ;
    dpv:hasSeverity risk:ExtremelyLowSeverity .

risk:RM7x7S1L5 a rdfs:Class,
        skos:Concept,
        risk:RiskAnalysis ;
    dct:contributor _:person-harshvardhan-j-pandit ;
    dct:created "2022-08-17"^^xsd:date ;
    rdf:value 0.10 ;
    rdfs:isDefinedBy risk: ;
    sw:term_status "accepted"@en ;
    skos:broader risk:RiskMatrix7x7 ;
    skos:definition "Node in a 7x7 Risk Matrix with Risk Severity: Extremely Low; Likelihood: High; and Risk Level: Very Low"@en ;
    skos:inScheme risk:risk-matrix-classes ;
    skos:prefLabel "Very Low Risk (RM7x7 S:1 L:5)"@en ;
    dpv:hasLikelihood risk:HighLikelihood ;
    dpv:hasRiskLevel risk:VeryLowRisk ;
    dpv:hasSeverity risk:ExtremelyLowSeverity .

risk:RM7x7S1L6 a rdfs:Class,
        skos:Concept,
        risk:RiskAnalysis ;
    dct:contributor _:person-harshvardhan-j-pandit ;
    dct:created "2022-08-17"^^xsd:date ;
    rdf:value 0.12 ;
    rdfs:isDefinedBy risk: ;
    sw:term_status "accepted"@en ;
    skos:broader risk:RiskMatrix7x7 ;
    skos:definition "Node in a 7x7 Risk Matrix with Risk Severity: Extremely Low; Likelihood: Very High; and Risk Level: Very Low"@en ;
    skos:inScheme risk:risk-matrix-classes ;
    skos:prefLabel "Very Low Risk (RM7x7 S:1 L:6)"@en ;
    dpv:hasLikelihood risk:VeryHighLikelihood ;
    dpv:hasRiskLevel risk:VeryLowRisk ;
    dpv:hasSeverity risk:ExtremelyLowSeverity .

risk:RM7x7S1L7 a rdfs:Class,
        skos:Concept,
        risk:RiskAnalysis ;
    dct:contributor _:person-harshvardhan-j-pandit ;
    dct:created "2022-08-17"^^xsd:date ;
    rdf:value 0.14 ;
    rdfs:isDefinedBy risk: ;
    sw:term_status "accepted"@en ;
    skos:broader risk:RiskMatrix7x7 ;
    skos:definition "Node in a 7x7 Risk Matrix with Risk Severity: Extremely Low; Likelihood: Extremely High; and Risk Level: Low"@en ;
    skos:inScheme risk:risk-matrix-classes ;
    skos:prefLabel "Low Risk (RM7x7 S:1 L:7)"@en ;
    dpv:hasLikelihood risk:ExtremelyHighLikelihood ;
    dpv:hasRiskLevel risk:LowRisk ;
    dpv:hasSeverity risk:ExtremelyLowSeverity .

risk:RM7x7S2L1 a rdfs:Class,
        skos:Concept,
        risk:RiskAnalysis ;
    dct:contributor _:person-harshvardhan-j-pandit ;
    dct:created "2022-08-17"^^xsd:date ;
    rdf:value 0.04 ;
    rdfs:isDefinedBy risk: ;
    sw:term_status "accepted"@en ;
    skos:broader risk:RiskMatrix7x7 ;
    skos:definition "Node in a 7x7 Risk Matrix with Risk Severity: Very Low; Likelihood: Extremely Low; and Risk Level: Extremely Low"@en ;
    skos:inScheme risk:risk-matrix-classes ;
    skos:prefLabel "Extremely Low Risk (RM7x7 S:2 L:1)"@en ;
    dpv:hasLikelihood risk:ExtremelyLowLikelihood ;
    dpv:hasRiskLevel risk:ExtremelyLowRisk ;
    dpv:hasSeverity risk:VeryLowSeverity .

risk:RM7x7S2L2 a rdfs:Class,
        skos:Concept,
        risk:RiskAnalysis ;
    dct:contributor _:person-harshvardhan-j-pandit ;
    dct:created "2022-08-17"^^xsd:date ;
    rdf:value 0.08 ;
    rdfs:isDefinedBy risk: ;
    sw:term_status "accepted"@en ;
    skos:broader risk:RiskMatrix7x7 ;
    skos:definition "Node in a 7x7 Risk Matrix with Risk Severity: Very Low; Likelihood: Very Low; and Risk Level: Extremely Low"@en ;
    skos:inScheme risk:risk-matrix-classes ;
    skos:prefLabel "Extremely Low Risk (RM7x7 S:2 L:2)"@en ;
    dpv:hasLikelihood risk:VeryLowLikelihood ;
    dpv:hasRiskLevel risk:ExtremelyLowRisk ;
    dpv:hasSeverity risk:VeryLowSeverity .

risk:RM7x7S2L3 a rdfs:Class,
        skos:Concept,
        risk:RiskAnalysis ;
    dct:contributor _:person-harshvardhan-j-pandit ;
    dct:created "2022-08-17"^^xsd:date ;
    rdf:value 0.12 ;
    rdfs:isDefinedBy risk: ;
    sw:term_status "accepted"@en ;
    skos:broader risk:RiskMatrix7x7 ;
    skos:definition "Node in a 7x7 Risk Matrix with Risk Severity: Very Low; Likelihood: Low; and Risk Level: Very Low"@en ;
    skos:inScheme risk:risk-matrix-classes ;
    skos:prefLabel "Very Low Risk (RM7x7 S:2 L:3)"@en ;
    dpv:hasLikelihood risk:LowLikelihood ;
    dpv:hasRiskLevel risk:VeryLowRisk ;
    dpv:hasSeverity risk:VeryLowSeverity .

risk:RM7x7S2L4 a rdfs:Class,
        skos:Concept,
        risk:RiskAnalysis ;
    dct:contributor _:person-harshvardhan-j-pandit ;
    dct:created "2022-08-17"^^xsd:date ;
    rdf:value 0.16 ;
    rdfs:isDefinedBy risk: ;
    sw:term_status "accepted"@en ;
    skos:broader risk:RiskMatrix7x7 ;
    skos:definition "Node in a 7x7 Risk Matrix with Risk Severity: Very Low; Likelihood: Moderate; and Risk Level: Low"@en ;
    skos:inScheme risk:risk-matrix-classes ;
    skos:prefLabel "Low Risk (RM7x7 S:2 L:4)"@en ;
    dpv:hasLikelihood risk:ModerateLikelihood ;
    dpv:hasRiskLevel risk:LowRisk ;
    dpv:hasSeverity risk:VeryLowSeverity .

risk:RM7x7S2L5 a rdfs:Class,
        skos:Concept,
        risk:RiskAnalysis ;
    dct:contributor _:person-harshvardhan-j-pandit ;
    dct:created "2022-08-17"^^xsd:date ;
    rdf:value 0.20 ;
    rdfs:isDefinedBy risk: ;
    sw:term_status "accepted"@en ;
    skos:broader risk:RiskMatrix7x7 ;
    skos:definition "Node in a 7x7 Risk Matrix with Risk Severity: Very Low; Likelihood: High; and Risk Level: Low"@en ;
    skos:inScheme risk:risk-matrix-classes ;
    skos:prefLabel "Low Risk (RM7x7 S:2 L:5)"@en ;
    dpv:hasLikelihood risk:HighLikelihood ;
    dpv:hasRiskLevel risk:LowRisk ;
    dpv:hasSeverity risk:VeryLowSeverity .

risk:RM7x7S2L6 a rdfs:Class,
        skos:Concept,
        risk:RiskAnalysis ;
    dct:contributor _:person-harshvardhan-j-pandit ;
    dct:created "2022-08-17"^^xsd:date ;
    rdf:value 0.24 ;
    rdfs:isDefinedBy risk: ;
    sw:term_status "accepted"@en ;
    skos:broader risk:RiskMatrix7x7 ;
    skos:definition "Node in a 7x7 Risk Matrix with Risk Severity: Very Low; Likelihood: Very High; and Risk Level: Moderate"@en ;
    skos:inScheme risk:risk-matrix-classes ;
    skos:prefLabel "Moderate Risk (RM7x7 S:2 L:6)"@en ;
    dpv:hasLikelihood risk:VeryHighLikelihood ;
    dpv:hasRiskLevel risk:ModerateRisk ;
    dpv:hasSeverity risk:VeryLowSeverity .

risk:RM7x7S2L7 a rdfs:Class,
        skos:Concept,
        risk:RiskAnalysis ;
    dct:contributor _:person-harshvardhan-j-pandit ;
    dct:created "2022-08-17"^^xsd:date ;
    rdf:value 0.29 ;
    rdfs:isDefinedBy risk: ;
    sw:term_status "accepted"@en ;
    skos:broader risk:RiskMatrix7x7 ;
    skos:definition "Node in a 7x7 Risk Matrix with Risk Severity: Very Low; Likelihood: Extremely High; and Risk Level: Moderate"@en ;
    skos:inScheme risk:risk-matrix-classes ;
    skos:prefLabel "Moderate Risk (RM7x7 S:2 L:7)"@en ;
    dpv:hasLikelihood risk:ExtremelyHighLikelihood ;
    dpv:hasRiskLevel risk:ModerateRisk ;
    dpv:hasSeverity risk:VeryLowSeverity .

risk:RM7x7S3L1 a rdfs:Class,
        skos:Concept,
        risk:RiskAnalysis ;
    dct:contributor _:person-harshvardhan-j-pandit ;
    dct:created "2022-08-17"^^xsd:date ;
    rdf:value 0.06 ;
    rdfs:isDefinedBy risk: ;
    sw:term_status "accepted"@en ;
    skos:broader risk:RiskMatrix7x7 ;
    skos:definition "Node in a 7x7 Risk Matrix with Risk Severity: Low; Likelihood: Extremely Low; and Risk Level: Extremely Low"@en ;
    skos:inScheme risk:risk-matrix-classes ;
    skos:prefLabel "Extremely Low Risk (RM7x7 S:3 L:1)"@en ;
    dpv:hasLikelihood risk:ExtremelyLowLikelihood ;
    dpv:hasRiskLevel risk:ExtremelyLowRisk ;
    dpv:hasSeverity risk:LowSeverity .

risk:RM7x7S3L2 a rdfs:Class,
        skos:Concept,
        risk:RiskAnalysis ;
    dct:contributor _:person-harshvardhan-j-pandit ;
    dct:created "2022-08-17"^^xsd:date ;
    rdf:value 0.12 ;
    rdfs:isDefinedBy risk: ;
    sw:term_status "accepted"@en ;
    skos:broader risk:RiskMatrix7x7 ;
    skos:definition "Node in a 7x7 Risk Matrix with Risk Severity: Low; Likelihood: Very Low; and Risk Level: Very Low"@en ;
    skos:inScheme risk:risk-matrix-classes ;
    skos:prefLabel "Very Low Risk (RM7x7 S:3 L:2)"@en ;
    dpv:hasLikelihood risk:VeryLowLikelihood ;
    dpv:hasRiskLevel risk:VeryLowRisk ;
    dpv:hasSeverity risk:LowSeverity .

risk:RM7x7S3L3 a rdfs:Class,
        skos:Concept,
        risk:RiskAnalysis ;
    dct:contributor _:person-harshvardhan-j-pandit ;
    dct:created "2022-08-17"^^xsd:date ;
    rdf:value 0.18 ;
    rdfs:isDefinedBy risk: ;
    sw:term_status "accepted"@en ;
    skos:broader risk:RiskMatrix7x7 ;
    skos:definition "Node in a 7x7 Risk Matrix with Risk Severity: Low; Likelihood: Low; and Risk Level: Low"@en ;
    skos:inScheme risk:risk-matrix-classes ;
    skos:prefLabel "Low Risk (RM7x7 S:3 L:3)"@en ;
    dpv:hasLikelihood risk:LowLikelihood ;
    dpv:hasRiskLevel risk:LowRisk ;
    dpv:hasSeverity risk:LowSeverity .

risk:RM7x7S3L4 a rdfs:Class,
        skos:Concept,
        risk:RiskAnalysis ;
    dct:contributor _:person-harshvardhan-j-pandit ;
    dct:created "2022-08-17"^^xsd:date ;
    rdf:value 0.24 ;
    rdfs:isDefinedBy risk: ;
    sw:term_status "accepted"@en ;
    skos:broader risk:RiskMatrix7x7 ;
    skos:definition "Node in a 7x7 Risk Matrix with Risk Severity: Low; Likelihood: Moderate; and Risk Level: Moderate"@en ;
    skos:inScheme risk:risk-matrix-classes ;
    skos:prefLabel "Moderate Risk (RM7x7 S:3 L:4)"@en ;
    dpv:hasLikelihood risk:ModerateLikelihood ;
    dpv:hasRiskLevel risk:ModerateRisk ;
    dpv:hasSeverity risk:LowSeverity .

risk:RM7x7S3L5 a rdfs:Class,
        skos:Concept,
        risk:RiskAnalysis ;
    dct:contributor _:person-harshvardhan-j-pandit ;
    dct:created "2022-08-17"^^xsd:date ;
    rdf:value 0.31 ;
    rdfs:isDefinedBy risk: ;
    sw:term_status "accepted"@en ;
    skos:broader risk:RiskMatrix7x7 ;
    skos:definition "Node in a 7x7 Risk Matrix with Risk Severity: Low; Likelihood: High; and Risk Level: High"@en ;
    skos:inScheme risk:risk-matrix-classes ;
    skos:prefLabel "High Risk (RM7x7 S:3 L:5)"@en ;
    dpv:hasLikelihood risk:HighLikelihood ;
    dpv:hasRiskLevel risk:HighRisk ;
    dpv:hasSeverity risk:LowSeverity .

risk:RM7x7S3L6 a rdfs:Class,
        skos:Concept,
        risk:RiskAnalysis ;
    dct:contributor _:person-harshvardhan-j-pandit ;
    dct:created "2022-08-17"^^xsd:date ;
    rdf:value 0.37 ;
    rdfs:isDefinedBy risk: ;
    sw:term_status "accepted"@en ;
    skos:broader risk:RiskMatrix7x7 ;
    skos:definition "Node in a 7x7 Risk Matrix with Risk Severity: Low; Likelihood: Very High; and Risk Level: High"@en ;
    skos:inScheme risk:risk-matrix-classes ;
    skos:prefLabel "High Risk (RM7x7 S:3 L:6)"@en ;
    dpv:hasLikelihood risk:VeryHighLikelihood ;
    dpv:hasRiskLevel risk:HighRisk ;
    dpv:hasSeverity risk:LowSeverity .

risk:RM7x7S3L7 a rdfs:Class,
        skos:Concept,
        risk:RiskAnalysis ;
    dct:contributor _:person-harshvardhan-j-pandit ;
    dct:created "2022-08-17"^^xsd:date ;
    rdf:value 0.43 ;
    rdfs:isDefinedBy risk: ;
    sw:term_status "accepted"@en ;
    skos:broader risk:RiskMatrix7x7 ;
    skos:definition "Node in a 7x7 Risk Matrix with Risk Severity: Low; Likelihood: Extremely High; and Risk Level: Very High"@en ;
    skos:inScheme risk:risk-matrix-classes ;
    skos:prefLabel "Very High Risk (RM7x7 S:3 L:7)"@en ;
    dpv:hasLikelihood risk:ExtremelyHighLikelihood ;
    dpv:hasRiskLevel risk:VeryHighRisk ;
    dpv:hasSeverity risk:LowSeverity .

risk:RM7x7S4L1 a rdfs:Class,
        skos:Concept,
        risk:RiskAnalysis ;
    dct:contributor _:person-harshvardhan-j-pandit ;
    dct:created "2022-08-17"^^xsd:date ;
    rdf:value 0.08 ;
    rdfs:isDefinedBy risk: ;
    sw:term_status "accepted"@en ;
    skos:broader risk:RiskMatrix7x7 ;
    skos:definition "Node in a 7x7 Risk Matrix with Risk Severity: Moderate; Likelihood: Extremely Low; and Risk Level: Extremely Low"@en ;
    skos:inScheme risk:risk-matrix-classes ;
    skos:prefLabel "Extremely Low Risk (RM7x7 S:4 L:1)"@en ;
    dpv:hasLikelihood risk:ExtremelyLowLikelihood ;
    dpv:hasRiskLevel risk:ExtremelyLowRisk ;
    dpv:hasSeverity risk:ModerateSeverity .

risk:RM7x7S4L2 a rdfs:Class,
        skos:Concept,
        risk:RiskAnalysis ;
    dct:contributor _:person-harshvardhan-j-pandit ;
    dct:created "2022-08-17"^^xsd:date ;
    rdf:value 0.16 ;
    rdfs:isDefinedBy risk: ;
    sw:term_status "accepted"@en ;
    skos:broader risk:RiskMatrix7x7 ;
    skos:definition "Node in a 7x7 Risk Matrix with Risk Severity: Moderate; Likelihood: Very Low; and Risk Level: Low"@en ;
    skos:inScheme risk:risk-matrix-classes ;
    skos:prefLabel "Low Risk (RM7x7 S:4 L:2)"@en ;
    dpv:hasLikelihood risk:VeryLowLikelihood ;
    dpv:hasRiskLevel risk:LowRisk ;
    dpv:hasSeverity risk:ModerateSeverity .

risk:RM7x7S4L3 a rdfs:Class,
        skos:Concept,
        risk:RiskAnalysis ;
    dct:contributor _:person-harshvardhan-j-pandit ;
    dct:created "2022-08-17"^^xsd:date ;
    rdf:value 0.24 ;
    rdfs:isDefinedBy risk: ;
    sw:term_status "accepted"@en ;
    skos:broader risk:RiskMatrix7x7 ;
    skos:definition "Node in a 7x7 Risk Matrix with Risk Severity: Moderate; Likelihood: Low; and Risk Level: Moderate"@en ;
    skos:inScheme risk:risk-matrix-classes ;
    skos:prefLabel "Moderate Risk (RM7x7 S:4 L:3)"@en ;
    dpv:hasLikelihood risk:LowLikelihood ;
    dpv:hasRiskLevel risk:ModerateRisk ;
    dpv:hasSeverity risk:ModerateSeverity .

risk:RM7x7S4L4 a rdfs:Class,
        skos:Concept,
        risk:RiskAnalysis ;
    dct:contributor _:person-harshvardhan-j-pandit ;
    dct:created "2022-08-17"^^xsd:date ;
    rdf:value 0.33 ;
    rdfs:isDefinedBy risk: ;
    sw:term_status "accepted"@en ;
    skos:broader risk:RiskMatrix7x7 ;
    skos:definition "Node in a 7x7 Risk Matrix with Risk Severity: Moderate; Likelihood: Moderate; and Risk Level: High"@en ;
    skos:inScheme risk:risk-matrix-classes ;
    skos:prefLabel "High Risk (RM7x7 S:4 L:4)"@en ;
    dpv:hasLikelihood risk:ModerateLikelihood ;
    dpv:hasRiskLevel risk:HighRisk ;
    dpv:hasSeverity risk:ModerateSeverity .

risk:RM7x7S4L5 a rdfs:Class,
        skos:Concept,
        risk:RiskAnalysis ;
    dct:contributor _:person-harshvardhan-j-pandit ;
    dct:created "2022-08-17"^^xsd:date ;
    rdf:value 0.41 ;
    rdfs:isDefinedBy risk: ;
    sw:term_status "accepted"@en ;
    skos:broader risk:RiskMatrix7x7 ;
    skos:definition "Node in a 7x7 Risk Matrix with Risk Severity: Moderate; Likelihood: High; and Risk Level: High"@en ;
    skos:inScheme risk:risk-matrix-classes ;
    skos:prefLabel "High Risk (RM7x7 S:4 L:5)"@en ;
    dpv:hasLikelihood risk:HighLikelihood ;
    dpv:hasRiskLevel risk:HighRisk ;
    dpv:hasSeverity risk:ModerateSeverity .

risk:RM7x7S4L6 a rdfs:Class,
        skos:Concept,
        risk:RiskAnalysis ;
    dct:contributor _:person-harshvardhan-j-pandit ;
    dct:created "2022-08-17"^^xsd:date ;
    rdf:value 0.49 ;
    rdfs:isDefinedBy risk: ;
    sw:term_status "accepted"@en ;
    skos:broader risk:RiskMatrix7x7 ;
    skos:definition "Node in a 7x7 Risk Matrix with Risk Severity: Moderate; Likelihood: Very High; and Risk Level: Very High"@en ;
    skos:inScheme risk:risk-matrix-classes ;
    skos:prefLabel "Very High Risk (RM7x7 S:4 L:6)"@en ;
    dpv:hasLikelihood risk:VeryHighLikelihood ;
    dpv:hasRiskLevel risk:VeryHighRisk ;
    dpv:hasSeverity risk:ModerateSeverity .

risk:RM7x7S4L7 a rdfs:Class,
        skos:Concept,
        risk:RiskAnalysis ;
    dct:contributor _:person-harshvardhan-j-pandit ;
    dct:created "2022-08-17"^^xsd:date ;
    rdf:value 0.57 ;
    rdfs:isDefinedBy risk: ;
    sw:term_status "accepted"@en ;
    skos:broader risk:RiskMatrix7x7 ;
    skos:definition "Node in a 7x7 Risk Matrix with Risk Severity: Moderate; Likelihood: Extremely High; and Risk Level: Very High"@en ;
    skos:inScheme risk:risk-matrix-classes ;
    skos:prefLabel "Very High Risk (RM7x7 S:4 L:7)"@en ;
    dpv:hasLikelihood risk:ExtremelyHighLikelihood ;
    dpv:hasRiskLevel risk:VeryHighRisk ;
    dpv:hasSeverity risk:ModerateSeverity .

risk:RM7x7S5L1 a rdfs:Class,
        skos:Concept,
        risk:RiskAnalysis ;
    dct:contributor _:person-harshvardhan-j-pandit ;
    dct:created "2022-08-17"^^xsd:date ;
    rdf:value 0.10 ;
    rdfs:isDefinedBy risk: ;
    sw:term_status "accepted"@en ;
    skos:broader risk:RiskMatrix7x7 ;
    skos:definition "Node in a 7x7 Risk Matrix with Risk Severity: High; Likelihood: Extremely Low; and Risk Level: Very Low"@en ;
    skos:inScheme risk:risk-matrix-classes ;
    skos:prefLabel "Very Low Risk (RM7x7 S:5 L:1)"@en ;
    dpv:hasLikelihood risk:ExtremelyLowLikelihood ;
    dpv:hasRiskLevel risk:VeryLowRisk ;
    dpv:hasSeverity risk:HighSeverity .

risk:RM7x7S5L2 a rdfs:Class,
        skos:Concept,
        risk:RiskAnalysis ;
    dct:contributor _:person-harshvardhan-j-pandit ;
    dct:created "2022-08-17"^^xsd:date ;
    rdf:value 0.20 ;
    rdfs:isDefinedBy risk: ;
    sw:term_status "accepted"@en ;
    skos:broader risk:RiskMatrix7x7 ;
    skos:definition "Node in a 7x7 Risk Matrix with Risk Severity: High; Likelihood: Very Low; and Risk Level: Low"@en ;
    skos:inScheme risk:risk-matrix-classes ;
    skos:prefLabel "Low Risk (RM7x7 S:5 L:2)"@en ;
    dpv:hasLikelihood risk:VeryLowLikelihood ;
    dpv:hasRiskLevel risk:LowRisk ;
    dpv:hasSeverity risk:HighSeverity .

risk:RM7x7S5L3 a rdfs:Class,
        skos:Concept,
        risk:RiskAnalysis ;
    dct:contributor _:person-harshvardhan-j-pandit ;
    dct:created "2022-08-17"^^xsd:date ;
    rdf:value 0.31 ;
    rdfs:isDefinedBy risk: ;
    sw:term_status "accepted"@en ;
    skos:broader risk:RiskMatrix7x7 ;
    skos:definition "Node in a 7x7 Risk Matrix with Risk Severity: High; Likelihood: Low; and Risk Level: Moderate"@en ;
    skos:inScheme risk:risk-matrix-classes ;
    skos:prefLabel "Moderate Risk (RM7x7 S:5 L:3)"@en ;
    dpv:hasLikelihood risk:LowLikelihood ;
    dpv:hasRiskLevel risk:ModerateRisk ;
    dpv:hasSeverity risk:HighSeverity .

risk:RM7x7S5L4 a rdfs:Class,
        skos:Concept,
        risk:RiskAnalysis ;
    dct:contributor _:person-harshvardhan-j-pandit ;
    dct:created "2022-08-17"^^xsd:date ;
    rdf:value 0.41 ;
    rdfs:isDefinedBy risk: ;
    sw:term_status "accepted"@en ;
    skos:broader risk:RiskMatrix7x7 ;
    skos:definition "Node in a 7x7 Risk Matrix with Risk Severity: High; Likelihood: Moderate; and Risk Level: High"@en ;
    skos:inScheme risk:risk-matrix-classes ;
    skos:prefLabel "High Risk (RM7x7 S:5 L:4)"@en ;
    dpv:hasLikelihood risk:ModerateLikelihood ;
    dpv:hasRiskLevel risk:HighRisk ;
    dpv:hasSeverity risk:HighSeverity .

risk:RM7x7S5L5 a rdfs:Class,
        skos:Concept,
        risk:RiskAnalysis ;
    dct:contributor _:person-harshvardhan-j-pandit ;
    dct:created "2022-08-17"^^xsd:date ;
    rdf:value 0.51 ;
    rdfs:isDefinedBy risk: ;
    sw:term_status "accepted"@en ;
    skos:broader risk:RiskMatrix7x7 ;
    skos:definition "Node in a 7x7 Risk Matrix with Risk Severity: High; Likelihood: High; and Risk Level: Very High"@en ;
    skos:inScheme risk:risk-matrix-classes ;
    skos:prefLabel "Very High Risk (RM7x7 S:5 L:5)"@en ;
    dpv:hasLikelihood risk:HighLikelihood ;
    dpv:hasRiskLevel risk:VeryHighRisk ;
    dpv:hasSeverity risk:HighSeverity .

risk:RM7x7S5L6 a rdfs:Class,
        skos:Concept,
        risk:RiskAnalysis ;
    dct:contributor _:person-harshvardhan-j-pandit ;
    dct:created "2022-08-17"^^xsd:date ;
    rdf:value 0.61 ;
    rdfs:isDefinedBy risk: ;
    sw:term_status "accepted"@en ;
    skos:broader risk:RiskMatrix7x7 ;
    skos:definition "Node in a 7x7 Risk Matrix with Risk Severity: High; Likelihood: Very High; and Risk Level: Extremely High"@en ;
    skos:inScheme risk:risk-matrix-classes ;
    skos:prefLabel "Extremely High Risk (RM7x7 S:5 L:6)"@en ;
    dpv:hasLikelihood risk:VeryHighLikelihood ;
    dpv:hasRiskLevel risk:ExtremelyHighRisk ;
    dpv:hasSeverity risk:HighSeverity .

risk:RM7x7S5L7 a rdfs:Class,
        skos:Concept,
        risk:RiskAnalysis ;
    dct:contributor _:person-harshvardhan-j-pandit ;
    dct:created "2022-08-17"^^xsd:date ;
    rdf:value 0.71 ;
    rdfs:isDefinedBy risk: ;
    sw:term_status "accepted"@en ;
    skos:broader risk:RiskMatrix7x7 ;
    skos:definition "Node in a 7x7 Risk Matrix with Risk Severity: High; Likelihood: Extremely High; and Risk Level: Extremely High"@en ;
    skos:inScheme risk:risk-matrix-classes ;
    skos:prefLabel "Extremely High Risk (RM7x7 S:5 L:7)"@en ;
    dpv:hasLikelihood risk:ExtremelyHighLikelihood ;
    dpv:hasRiskLevel risk:ExtremelyHighRisk ;
    dpv:hasSeverity risk:HighSeverity .

risk:RM7x7S6L1 a rdfs:Class,
        skos:Concept,
        risk:RiskAnalysis ;
    dct:contributor _:person-harshvardhan-j-pandit ;
    dct:created "2022-08-17"^^xsd:date ;
    rdf:value 0.12 ;
    rdfs:isDefinedBy risk: ;
    sw:term_status "accepted"@en ;
    skos:broader risk:RiskMatrix7x7 ;
    skos:definition "Node in a 7x7 Risk Matrix with Risk Severity: Very High; Likelihood: Extremely Low; and Risk Level: Very Low"@en ;
    skos:inScheme risk:risk-matrix-classes ;
    skos:prefLabel "Very Low Risk (RM7x7 S:6 L:1)"@en ;
    dpv:hasLikelihood risk:ExtremelyLowLikelihood ;
    dpv:hasRiskLevel risk:VeryLowRisk ;
    dpv:hasSeverity risk:VeryHighSeverity .

risk:RM7x7S6L2 a rdfs:Class,
        skos:Concept,
        risk:RiskAnalysis ;
    dct:contributor _:person-harshvardhan-j-pandit ;
    dct:created "2022-08-17"^^xsd:date ;
    rdf:value 0.24 ;
    rdfs:isDefinedBy risk: ;
    sw:term_status "accepted"@en ;
    skos:broader risk:RiskMatrix7x7 ;
    skos:definition "Node in a 7x7 Risk Matrix with Risk Severity: Very High; Likelihood: Very Low; and Risk Level: Moderate"@en ;
    skos:inScheme risk:risk-matrix-classes ;
    skos:prefLabel "Moderate Risk (RM7x7 S:6 L:2)"@en ;
    dpv:hasLikelihood risk:VeryLowLikelihood ;
    dpv:hasRiskLevel risk:ModerateRisk ;
    dpv:hasSeverity risk:VeryHighSeverity .

risk:RM7x7S6L3 a rdfs:Class,
        skos:Concept,
        risk:RiskAnalysis ;
    dct:contributor _:person-harshvardhan-j-pandit ;
    dct:created "2022-08-17"^^xsd:date ;
    rdf:value 0.37 ;
    rdfs:isDefinedBy risk: ;
    sw:term_status "accepted"@en ;
    skos:broader risk:RiskMatrix7x7 ;
    skos:definition "Node in a 7x7 Risk Matrix with Risk Severity: Very High; Likelihood: Low; and Risk Level: High"@en ;
    skos:inScheme risk:risk-matrix-classes ;
    skos:prefLabel "High Risk (RM7x7 S:6 L:3)"@en ;
    dpv:hasLikelihood risk:LowLikelihood ;
    dpv:hasRiskLevel risk:HighRisk ;
    dpv:hasSeverity risk:VeryHighSeverity .

risk:RM7x7S6L4 a rdfs:Class,
        skos:Concept,
        risk:RiskAnalysis ;
    dct:contributor _:person-harshvardhan-j-pandit ;
    dct:created "2022-08-17"^^xsd:date ;
    rdf:value 0.49 ;
    rdfs:isDefinedBy risk: ;
    sw:term_status "accepted"@en ;
    skos:broader risk:RiskMatrix7x7 ;
    skos:definition "Node in a 7x7 Risk Matrix with Risk Severity: Very High; Likelihood: Moderate; and Risk Level: Very High"@en ;
    skos:inScheme risk:risk-matrix-classes ;
    skos:prefLabel "Very High Risk (RM7x7 S:6 L:4)"@en ;
    dpv:hasLikelihood risk:ModerateLikelihood ;
    dpv:hasRiskLevel risk:VeryHighRisk ;
    dpv:hasSeverity risk:VeryHighSeverity .

risk:RM7x7S6L5 a rdfs:Class,
        skos:Concept,
        risk:RiskAnalysis ;
    dct:contributor _:person-harshvardhan-j-pandit ;
    dct:created "2022-08-17"^^xsd:date ;
    rdf:value 0.61 ;
    rdfs:isDefinedBy risk: ;
    sw:term_status "accepted"@en ;
    skos:broader risk:RiskMatrix7x7 ;
    skos:definition "Node in a 7x7 Risk Matrix with Risk Severity: Very High; Likelihood: High; and Risk Level: Very High"@en ;
    skos:inScheme risk:risk-matrix-classes ;
    skos:prefLabel "Very High Risk (RM7x7 S:6 L:5)"@en ;
    dpv:hasLikelihood risk:HighLikelihood ;
    dpv:hasRiskLevel risk:VeryHighRisk ;
    dpv:hasSeverity risk:VeryHighSeverity .

risk:RM7x7S6L6 a rdfs:Class,
        skos:Concept,
        risk:RiskAnalysis ;
    dct:contributor _:person-harshvardhan-j-pandit ;
    dct:created "2022-08-17"^^xsd:date ;
    rdf:value 0.73 ;
    rdfs:isDefinedBy risk: ;
    sw:term_status "accepted"@en ;
    skos:broader risk:RiskMatrix7x7 ;
    skos:definition "Node in a 7x7 Risk Matrix with Risk Severity: Very High; Likelihood: Very High; and Risk Level: Extremely High"@en ;
    skos:inScheme risk:risk-matrix-classes ;
    skos:prefLabel "Extremely High Risk (RM7x7 S:6 L:6)"@en ;
    dpv:hasLikelihood risk:VeryHighLikelihood ;
    dpv:hasRiskLevel risk:ExtremelyHighRisk ;
    dpv:hasSeverity risk:VeryHighSeverity .

risk:RM7x7S6L7 a rdfs:Class,
        skos:Concept,
        risk:RiskAnalysis ;
    dct:contributor _:person-harshvardhan-j-pandit ;
    dct:created "2022-08-17"^^xsd:date ;
    rdf:value 0.86 ;
    rdfs:isDefinedBy risk: ;
    sw:term_status "accepted"@en ;
    skos:broader risk:RiskMatrix7x7 ;
    skos:definition "Node in a 7x7 Risk Matrix with Risk Severity: Very High; Likelihood: Extremely High; and Risk Level: Extremely High"@en ;
    skos:inScheme risk:risk-matrix-classes ;
    skos:prefLabel "Extremely High Risk (RM7x7 S:6 L:7)"@en ;
    dpv:hasLikelihood risk:ExtremelyHighLikelihood ;
    dpv:hasRiskLevel risk:ExtremelyHighRisk ;
    dpv:hasSeverity risk:VeryHighSeverity .

risk:RM7x7S7L1 a rdfs:Class,
        skos:Concept,
        risk:RiskAnalysis ;
    dct:contributor _:person-harshvardhan-j-pandit ;
    dct:created "2022-08-17"^^xsd:date ;
    rdf:value 0.14 ;
    rdfs:isDefinedBy risk: ;
    sw:term_status "accepted"@en ;
    skos:broader risk:RiskMatrix7x7 ;
    skos:definition "Node in a 7x7 Risk Matrix with Risk Severity: Extremely High; Likelihood: Extremely Low; and Risk Level: Low"@en ;
    skos:inScheme risk:risk-matrix-classes ;
    skos:prefLabel "Low Risk (RM7x7 S:7 L:1)"@en ;
    dpv:hasLikelihood risk:ExtremelyLowLikelihood ;
    dpv:hasRiskLevel risk:LowRisk ;
    dpv:hasSeverity risk:ExtremelyHighSeverity .

risk:RM7x7S7L2 a rdfs:Class,
        skos:Concept,
        risk:RiskAnalysis ;
    dct:contributor _:person-harshvardhan-j-pandit ;
    dct:created "2022-08-17"^^xsd:date ;
    rdf:value 0.29 ;
    rdfs:isDefinedBy risk: ;
    sw:term_status "accepted"@en ;
    skos:broader risk:RiskMatrix7x7 ;
    skos:definition "Node in a 7x7 Risk Matrix with Risk Severity: Extremely High; Likelihood: Very Low; and Risk Level: Moderate"@en ;
    skos:inScheme risk:risk-matrix-classes ;
    skos:prefLabel "Moderate Risk (RM7x7 S:7 L:2)"@en ;
    dpv:hasLikelihood risk:VeryLowLikelihood ;
    dpv:hasRiskLevel risk:ModerateRisk ;
    dpv:hasSeverity risk:ExtremelyHighSeverity .

risk:RM7x7S7L3 a rdfs:Class,
        skos:Concept,
        risk:RiskAnalysis ;
    dct:contributor _:person-harshvardhan-j-pandit ;
    dct:created "2022-08-17"^^xsd:date ;
    rdf:value 0.43 ;
    rdfs:isDefinedBy risk: ;
    sw:term_status "accepted"@en ;
    skos:broader risk:RiskMatrix7x7 ;
    skos:definition "Node in a 7x7 Risk Matrix with Risk Severity: Extremely High; Likelihood: Low; and Risk Level: High"@en ;
    skos:inScheme risk:risk-matrix-classes ;
    skos:prefLabel "High Risk (RM7x7 S:7 L:3)"@en ;
    dpv:hasLikelihood risk:LowLikelihood ;
    dpv:hasRiskLevel risk:HighRisk ;
    dpv:hasSeverity risk:ExtremelyHighSeverity .

risk:RM7x7S7L4 a rdfs:Class,
        skos:Concept,
        risk:RiskAnalysis ;
    dct:contributor _:person-harshvardhan-j-pandit ;
    dct:created "2022-08-17"^^xsd:date ;
    rdf:value 0.57 ;
    rdfs:isDefinedBy risk: ;
    sw:term_status "accepted"@en ;
    skos:broader risk:RiskMatrix7x7 ;
    skos:definition "Node in a 7x7 Risk Matrix with Risk Severity: Extremely High; Likelihood: Moderate; and Risk Level: Very High"@en ;
    skos:inScheme risk:risk-matrix-classes ;
    skos:prefLabel "Very High Risk (RM7x7 S:7 L:4)"@en ;
    dpv:hasLikelihood risk:ModerateLikelihood ;
    dpv:hasRiskLevel risk:VeryHighRisk ;
    dpv:hasSeverity risk:ExtremelyHighSeverity .

risk:RM7x7S7L5 a rdfs:Class,
        skos:Concept,
        risk:RiskAnalysis ;
    dct:contributor _:person-harshvardhan-j-pandit ;
    dct:created "2022-08-17"^^xsd:date ;
    rdf:value 0.71 ;
    rdfs:isDefinedBy risk: ;
    sw:term_status "accepted"@en ;
    skos:broader risk:RiskMatrix7x7 ;
    skos:definition "Node in a 7x7 Risk Matrix with Risk Severity: Extremely High; Likelihood: High; and Risk Level: Extremely High"@en ;
    skos:inScheme risk:risk-matrix-classes ;
    skos:prefLabel "Extremely High Risk (RM7x7 S:7 L:5)"@en ;
    dpv:hasLikelihood risk:HighLikelihood ;
    dpv:hasRiskLevel risk:ExtremelyHighRisk ;
    dpv:hasSeverity risk:ExtremelyHighSeverity .

risk:RM7x7S7L6 a rdfs:Class,
        skos:Concept,
        risk:RiskAnalysis ;
    dct:contributor _:person-harshvardhan-j-pandit ;
    dct:created "2022-08-17"^^xsd:date ;
    rdf:value 0.86 ;
    rdfs:isDefinedBy risk: ;
    sw:term_status "accepted"@en ;
    skos:broader risk:RiskMatrix7x7 ;
    skos:definition "Node in a 7x7 Risk Matrix with Risk Severity: Extremely High; Likelihood: Very High; and Risk Level: Extremely High"@en ;
    skos:inScheme risk:risk-matrix-classes ;
    skos:prefLabel "Extremely High Risk (RM7x7 S:7 L:6)"@en ;
    dpv:hasLikelihood risk:VeryHighLikelihood ;
    dpv:hasRiskLevel risk:ExtremelyHighRisk ;
    dpv:hasSeverity risk:ExtremelyHighSeverity .

risk:RM7x7S7L7 a rdfs:Class,
        skos:Concept,
        risk:RiskAnalysis ;
    dct:contributor _:person-harshvardhan-j-pandit ;
    dct:created "2022-08-17"^^xsd:date ;
    rdf:value 0.99 ;
    rdfs:isDefinedBy risk: ;
    sw:term_status "accepted"@en ;
    skos:broader risk:RiskMatrix7x7 ;
    skos:definition "Node in a 7x7 Risk Matrix with Risk Severity: Extremely High; Likelihood: Extremely High; and Risk Level: Extremely High"@en ;
    skos:inScheme risk:risk-matrix-classes ;
    skos:prefLabel "Extremely High Risk (RM7x7 S:7 L:7)"@en ;
    dpv:hasLikelihood risk:ExtremelyHighLikelihood ;
    dpv:hasRiskLevel risk:ExtremelyHighRisk ;
    dpv:hasSeverity risk:ExtremelyHighSeverity .

risk:RacialDiscrimination a rdfs:Class,
        skos:Concept,
        dpv:RiskConcept,
        risk:PotentialConsequence,
        risk:PotentialImpact,
        risk:PotentialRisk ;
    dct:created "2024-09-30"^^xsd:date ;
    rdfs:isDefinedBy risk: ;
    sw:term_status "accepted"@en ;
    skos:broader risk:Racism ;
    skos:definition "Discrimination against individuals because of their racial background or skin colour"@en ;
    skos:inScheme risk:risk-taxonomy-classes ;
    skos:prefLabel "Racial Discrimination"@en .

risk:Racism a rdfs:Class,
        skos:Concept,
        dpv:RiskConcept,
        risk:PotentialConsequence,
        risk:PotentialImpact,
        risk:PotentialRisk ;
    dct:created "2024-09-30"^^xsd:date ;
    rdfs:isDefinedBy risk: ;
    sw:term_status "accepted"@en ;
    skos:broader risk:Discrimination ;
    skos:definition "Prejudice or discrimination against people based on their race"@en ;
    skos:inScheme risk:risk-taxonomy-classes ;
    skos:prefLabel "Racism"@en .

risk:ReactiveControl a rdfs:Class,
        skos:Concept,
        risk:RiskControl ;
    dct:contributor _:person-harshvardhan-j-pandit ;
    dct:created "2025-01-06"^^xsd:date ;
    rdfs:isDefinedBy risk: ;
    sw:term_status "accepted"@en ;
    skos:broader risk:RiskControl ;
    skos:definition "Control that is established or functions after an event occurs"@en ;
    skos:inScheme risk:risk-controls-classes ;
    skos:prefLabel "Reactive Control"@en ;
    skos:scopeNote "The use of 'reactive' here refers to this control being established i.e. becoming active to address the effects of an event after they occur. It does not imply that the controls are put in place after the event or that there is no planned procedure for handling an incident"@en .

risk:RecoveryControl a rdfs:Class,
        skos:Concept,
        risk:RiskControl ;
    dct:contributor _:person-delaram-golpayegani,
        _:person-harshvardhan-j-pandit ;
    dct:created "2024-05-19"^^xsd:date ;
    dct:modified "2025-01-06"^^xsd:date ;
    rdfs:isDefinedBy risk: ;
    sw:term_status "modified"@en ;
    skos:broader risk:ResolutionControl ;
    skos:definition "Control that aims to restore the context following an event"@en ;
    skos:inScheme risk:risk-controls-classes ;
    skos:prefLabel "Recovery Control"@en ;
    skos:scopeNote "Recovery implies taking steps to correct the effects which may not be the same as the initial conditions before the event, whereas risk:ReversalControl refers to undoing the effects such that the initial condition is restored"@en .

risk:ReduceLikelihood a rdfs:Class,
        skos:Concept,
        risk:RiskControl ;
    dct:contributor _:person-harshvardhan-j-pandit ;
    dct:created "2024-05-19"^^xsd:date ;
    dct:modified "2025-01-06"^^xsd:date ;
    rdfs:isDefinedBy risk: ;
    sw:term_status "modified"@en ;
    skos:broader risk:ReductionControl ;
    skos:definition "Control that reduces the likelihood of an event to occur"@en ;
    skos:inScheme risk:risk-controls-classes ;
    skos:prefLabel "Reduce Likelihood"@en .

risk:ReduceSeverity a rdfs:Class,
        skos:Concept,
        risk:RiskControl ;
    dct:contributor _:person-harshvardhan-j-pandit ;
    dct:created "2024-05-19"^^xsd:date ;
    dct:modified "2025-01-06"^^xsd:date ;
    rdfs:isDefinedBy risk: ;
    sw:term_status "modified"@en ;
    skos:broader risk:ReductionControl ;
    skos:definition "Control that reduces the severity of an event's effects"@en ;
    skos:inScheme risk:risk-controls-classes ;
    skos:prefLabel "Reduce Severity"@en .

risk:ReductionControl a rdfs:Class,
        skos:Concept,
        risk:RiskControl ;
    dct:created "2024-05-19"^^xsd:date ;
    dct:modified "2025-01-06"^^xsd:date ;
    rdfs:isDefinedBy risk: ;
    sw:term_status "modified"@en ;
    skos:broader risk:ReactiveControl ;
    skos:definition "Control that reduces the effects of an event"@en ;
    skos:inScheme risk:risk-controls-classes ;
    skos:prefLabel "Reduction Control"@en ;
    skos:scopeNote "Reduction here refers to a lessening of the effects after the event has occurred by either reducing their likelihood or their severity in the context. This can involve changing the underlying context such that the effects have a reduced chance of occurring, or to create additional measures such that the effects do not have the initial severity for an entity"@en .

risk:Reidentification a rdfs:Class,
        skos:Concept,
        dpv:RiskConcept,
        risk:ConfidentialityConcept,
        risk:PotentialConsequence,
        risk:PotentialRisk,
        risk:PotentialRiskSource ;
    dct:contributor _:person-harshvardhan-j-pandit ;
    dct:created "2022-08-19"^^xsd:date ;
    dct:modified "2024-08-16"^^xsd:date ;
    rdfs:isDefinedBy risk: ;
    sw:term_status "accepted"@en ;
    skos:broader risk:OperationalSecurityRisk ;
    skos:definition "Concept representing Re-identification"@en ;
    skos:inScheme risk:risk-taxonomy-classes ;
    skos:prefLabel "Re-identification"@en ;
    skos:scopeNote "Use this concept for reidentification in an internal context. For reidentification performed by external entities see concept UnauthorisedReidentification"@en .

risk:ReligiousDiscrimination a rdfs:Class,
        skos:Concept,
        dpv:RiskConcept,
        risk:PotentialConsequence,
        risk:PotentialImpact,
        risk:PotentialRisk ;
    dct:created "2024-09-30"^^xsd:date ;
    rdfs:isDefinedBy risk: ;
    sw:term_status "accepted"@en ;
    skos:broader risk:Discrimination ;
    skos:definition "Discrimination based on a person's religion or religious beliefs or practices"@en ;
    skos:inScheme risk:risk-taxonomy-classes ;
    skos:prefLabel "Religious Discrimination"@en .

risk:RemediationControl a rdfs:Class,
        skos:Concept,
        risk:RiskControl ;
    dct:contributor _:person-arthit-suriyawongkul,
        _:person-delaram-golpayegani,
        _:person-harshvardhan-j-pandit ;
    dct:created "2024-05-19"^^xsd:date ;
    dct:modified "2025-08-06"^^xsd:date ;
    rdfs:isDefinedBy risk: ;
    sw:term_status "modified"@en ;
    skos:broader risk:ResolutionControl ;
    skos:definition "Control that aims to fix or remedy the causes of an event to prevent further occurrences"@en ;
    skos:inScheme risk:risk-controls-classes ;
    skos:prefLabel "Remediation Control"@en ;
    skos:scopeNote "Remediation involves making changes in the context to avoid further events and effects, which may be for the specific event or for other similar events and effects. As such, remediation can also be undertaken as a proactive measure in the risk management lifecycle following an incident"@en .

risk:RemoveConsequence a rdfs:Class,
        skos:Concept,
        risk:RiskControl ;
    dct:contributor _:person-harshvardhan-j-pandit ;
    dct:created "2024-05-19"^^xsd:date ;
    dct:modified "2025-01-06"^^xsd:date ;
    rdfs:isDefinedBy risk: ;
    sw:term_status "modified"@en ;
    skos:broader risk:ConsequenceControl,
        risk:EliminationControl ;
    skos:definition "Control that proactively removes the consequence event such that the event does not occur in the context"@en ;
    skos:inScheme risk:risk-controls-classes ;
    skos:prefLabel "Remove Consequence"@en .

risk:RemoveImpact a rdfs:Class,
        skos:Concept,
        risk:RiskControl ;
    dct:contributor _:person-harshvardhan-j-pandit ;
    dct:created "2024-05-19"^^xsd:date ;
    dct:modified "2025-01-06"^^xsd:date ;
    rdfs:isDefinedBy risk: ;
    sw:term_status "modified"@en ;
    skos:broader risk:EliminationControl,
        risk:ImpactControl ;
    skos:definition "Control that proactively removes the impact event such that the event does not occur in the context"@en ;
    skos:inScheme risk:risk-controls-classes ;
    skos:prefLabel "Remove Impact"@en .

risk:RemoveSource a rdfs:Class,
        skos:Concept,
        risk:RiskControl ;
    dct:contributor _:person-harshvardhan-j-pandit ;
    dct:created "2024-05-19"^^xsd:date ;
    dct:modified "2025-01-06"^^xsd:date ;
    rdfs:isDefinedBy risk: ;
    sw:term_status "modified"@en ;
    skos:broader risk:EliminationControl,
        risk:SourceControl ;
    skos:definition "Control that proactively removes the risk source such that it is no longer present or applicable in the context"@en ;
    skos:inScheme risk:risk-controls-classes ;
    skos:prefLabel "Remove Source"@en .

risk:Remuneration a rdfs:Class,
        skos:Concept,
        dpv:RiskConcept,
        risk:PotentialConsequence,
        risk:PotentialImpact,
        risk:PotentialRisk ;
    dct:contributor _:person-georg-p-krog,
        _:person-harshvardhan-j-pandit ;
    dct:created "2024-04-14"^^xsd:date ;
    dct:modified "2024-08-16"^^xsd:date ;
    rdfs:isDefinedBy risk: ;
    sw:term_status "accepted"@en ;
    skos:broader risk:FinancialImpact ;
    skos:definition "Something that acts as or provides remuneration which is in monetary or financial form"@en ;
    skos:inScheme risk:risk-taxonomy-classes ;
    skos:prefLabel "Remuneration"@en .

risk:ReputationalLoss a rdfs:Class,
        skos:Concept,
        dpv:RiskConcept,
        risk:PotentialConsequence,
        risk:PotentialImpact,
        risk:PotentialRisk ;
    dct:contributor _:person-harshvardhan-j-pandit ;
    dct:created "2022-08-17"^^xsd:date ;
    dct:modified "2025-08-27"^^xsd:date ;
    dct:source _:b15886bc6e88dcdb258fe59ded7be3abf ;
    rdfs:isDefinedBy risk: ;
    sw:term_status "modified"@en ;
    skos:broader risk:ReputationalRisk ;
    skos:definition "Concept representing Reputational Loss"@en ;
    skos:inScheme risk:risk-taxonomy-classes ;
    skos:prefLabel "Reputational Loss"@en .

risk:ReputationalRisk a rdfs:Class,
        skos:Concept,
        dpv:RiskConcept,
        risk:PotentialConsequence,
        risk:PotentialImpact,
        risk:PotentialRisk ;
    dct:created "2024-12-17"^^xsd:date ;
    rdfs:isDefinedBy risk: ;
    sw:term_status "accepted"@en ;
    skos:broader risk:OrganisationalRiskConcept ;
    skos:definition "Risks and issues that affect the reputation of the organisation"@en ;
    skos:inScheme risk:risk-taxonomy-classes ;
    skos:prefLabel "Reputational Risk"@en .

risk:RequirementsBias a rdfs:Class,
        skos:Concept,
        dpv:RiskConcept,
        risk:PotentialConsequence,
        risk:PotentialRisk,
        risk:PotentialRiskSource ;
    dct:contributor _:person-daniel-doherty,
        _:person-delaram-golpayegani,
        _:person-harshvardhan-j-pandit ;
    dct:created "2024-09-13"^^xsd:date ;
    dct:source "ISO/IEC 24027:2021"@en ;
    rdfs:isDefinedBy risk: ;
    sw:term_status "accepted"@en ;
    skos:broader risk:CognitiveBias ;
    skos:definition "Bias that occurs in or during requirements creation"@en ;
    skos:inScheme risk:risk-taxonomy-classes ;
    skos:prefLabel "Requirements Bias"@en ;
    skos:scopeNote "Requirements bias also represents occasions for the human cognitive biases to manifest"@en .

risk:ResilienceDegraded a rdfs:Class,
        skos:Concept,
        dpv:RiskConcept,
        risk:PotentialConsequence,
        risk:PotentialRisk,
        risk:PotentialRiskSource ;
    dct:contributor _:person-delaram-golpayegani,
        _:person-harshvardhan-j-pandit ;
    dct:created "2026-02-09"^^xsd:date ;
    rdfs:isDefinedBy risk: ;
    sw:term_status "accepted"@en ;
    skos:broader risk:QualityDegraded,
        risk:ResilienceRisk ;
    skos:definition "Concepts representing risks and issues where Resilience is Degraded"@en ;
    skos:inScheme risk:risk-taxonomy-classes ;
    skos:prefLabel "Resilience Degraded"@en .

risk:ResilienceInconsistent a rdfs:Class,
        skos:Concept,
        dpv:RiskConcept,
        risk:PotentialConsequence,
        risk:PotentialRisk,
        risk:PotentialRiskSource ;
    dct:contributor _:person-delaram-golpayegani,
        _:person-harshvardhan-j-pandit ;
    dct:created "2026-02-09"^^xsd:date ;
    rdfs:isDefinedBy risk: ;
    sw:term_status "accepted"@en ;
    skos:broader risk:QualityInconsistent,
        risk:ResilienceRisk ;
    skos:definition "Concepts representing risks and issues where Resilience is Inconsistent"@en ;
    skos:inScheme risk:risk-taxonomy-classes ;
    skos:prefLabel "Resilience Inconsistent"@en .

risk:ResilienceInsufficient a rdfs:Class,
        skos:Concept,
        dpv:RiskConcept,
        risk:PotentialConsequence,
        risk:PotentialRisk,
        risk:PotentialRiskSource ;
    dct:contributor _:person-delaram-golpayegani,
        _:person-harshvardhan-j-pandit ;
    dct:created "2026-02-09"^^xsd:date ;
    rdfs:isDefinedBy risk: ;
    sw:term_status "accepted"@en ;
    skos:broader risk:QualityInsufficient,
        risk:ResilienceRisk ;
    skos:definition "Concepts representing risks and issues where Resilience is Insufficient"@en ;
    skos:inScheme risk:risk-taxonomy-classes ;
    skos:prefLabel "Resilience Insufficient"@en .

risk:ResilienceRisk a rdfs:Class,
        skos:Concept,
        dpv:RiskConcept,
        risk:PotentialConsequence,
        risk:PotentialRisk,
        risk:PotentialRiskSource ;
    dct:contributor _:person-delaram-golpayegani,
        _:person-harshvardhan-j-pandit ;
    dct:created "2026-02-09"^^xsd:date ;
    rdfs:isDefinedBy risk: ;
    sw:term_status "accepted"@en ;
    skos:broader risk:QualityRisk ;
    skos:definition "Concepts representing risks and issues regarding Resilience"@en ;
    skos:inScheme risk:risk-taxonomy-classes ;
    skos:prefLabel "Resilience Risk"@en .

risk:ResilienceUnknown a rdfs:Class,
        skos:Concept,
        dpv:RiskConcept,
        risk:PotentialConsequence,
        risk:PotentialRisk,
        risk:PotentialRiskSource ;
    dct:contributor _:person-delaram-golpayegani,
        _:person-harshvardhan-j-pandit ;
    dct:created "2026-02-09"^^xsd:date ;
    rdfs:isDefinedBy risk: ;
    sw:term_status "accepted"@en ;
    skos:broader risk:QualityUnknown,
        risk:ResilienceRisk ;
    skos:definition "Concepts representing risks and issues where Resilience is Unknown"@en ;
    skos:inScheme risk:risk-taxonomy-classes ;
    skos:prefLabel "Resilience Unknown"@en .

risk:ResilienceUnverified a rdfs:Class,
        skos:Concept,
        dpv:RiskConcept,
        risk:PotentialConsequence,
        risk:PotentialRisk,
        risk:PotentialRiskSource ;
    dct:contributor _:person-delaram-golpayegani,
        _:person-harshvardhan-j-pandit ;
    dct:created "2026-02-09"^^xsd:date ;
    rdfs:isDefinedBy risk: ;
    sw:term_status "accepted"@en ;
    skos:broader risk:QualityUnverified,
        risk:ResilienceRisk ;
    skos:definition "Concepts representing risks and issues where Resilience is Unverified"@en ;
    skos:inScheme risk:risk-taxonomy-classes ;
    skos:prefLabel "Resilience Unverified"@en .

risk:ResolutionControl a rdfs:Class,
        skos:Concept,
        risk:RiskControl ;
    dct:contributor _:person-harshvardhan-j-pandit ;
    dct:created "2025-01-06"^^xsd:date ;
    rdfs:isDefinedBy risk: ;
    sw:term_status "accepted"@en ;
    skos:broader risk:ReactiveControl ;
    skos:definition "Control that aims to resolve an event's effects with the goal of fixing or recovering from it"@en ;
    skos:inScheme risk:risk-controls-classes ;
    skos:prefLabel "Resolution Control"@en .

risk:ReversalControl a rdfs:Class,
        skos:Concept,
        risk:RiskControl ;
    dct:contributor _:person-delaram-golpayegani,
        _:person-harshvardhan-j-pandit ;
    dct:created "2025-01-06"^^xsd:date ;
    rdfs:isDefinedBy risk: ;
    sw:term_status "accepted"@en ;
    skos:broader risk:ResolutionControl ;
    skos:definition "Control that aims to reverse or undo the effects of an event"@en ;
    skos:inScheme risk:risk-controls-classes ;
    skos:prefLabel "Reversal Control"@en ;
    skos:scopeNote "Reversal can be achieved through measures such as restoring information from a backup or replacing things such that the initial context not containing the event's effects is restored"@en .

risk:ReverseDiscrimination a rdfs:Class,
        skos:Concept,
        dpv:RiskConcept,
        risk:PotentialConsequence,
        risk:PotentialImpact,
        risk:PotentialRisk ;
    dct:created "2024-09-30"^^xsd:date ;
    rdfs:isDefinedBy risk: ;
    sw:term_status "accepted"@en ;
    skos:broader risk:Discrimination ;
    skos:definition "Discrimination against members of a majority or historically dominant group, often in the context of efforts to promote equality"@en ;
    skos:inScheme risk:risk-taxonomy-classes ;
    skos:prefLabel "Reverse Discrimination"@en .

risk:Reward a rdfs:Class,
        skos:Concept,
        dpv:RiskConcept,
        risk:PotentialConsequence,
        risk:PotentialImpact,
        risk:PotentialRisk ;
    dct:contributor _:person-georg-p-krog,
        _:person-harshvardhan-j-pandit ;
    dct:created "2024-04-14"^^xsd:date ;
    dct:modified "2025-08-06"^^xsd:date ;
    rdfs:isDefinedBy risk: ;
    sw:term_status "modified"@en ;
    skos:broader risk:Remuneration ;
    skos:definition "Something that acts as or provides rewards i.e. a benefit given for some service or activity that is not a payment or fee"@en ;
    skos:inScheme risk:risk-taxonomy-classes ;
    skos:prefLabel "Reward"@en .

risk:RightsDenied a rdfs:Class,
        skos:Concept,
        dpv:RiskConcept,
        risk:PotentialConsequence,
        risk:PotentialImpact,
        risk:PotentialRisk ;
    dct:created "2024-12-17"^^xsd:date ;
    rdfs:isDefinedBy risk: ;
    sw:term_status "accepted"@en ;
    skos:broader risk:RightsImpact ;
    skos:definition "The refusal or withholding or denial of the existence or applicability of rights"@en ;
    skos:inScheme risk:risk-taxonomy-classes ;
    skos:prefLabel "Rights Denied"@en ;
    skos:scopeNote "The denial of the right refers to the argument that a right does not apply at all for a particular case. Though specified as a plural i.e. 'rights', this concept can be applied to a singular right"@en .

risk:RightsEroded a rdfs:Class,
        skos:Concept,
        dpv:RiskConcept,
        risk:PotentialConsequence,
        risk:PotentialImpact,
        risk:PotentialRisk ;
    dct:created "2024-12-17"^^xsd:date ;
    rdfs:isDefinedBy risk: ;
    sw:term_status "accepted"@en ;
    skos:broader risk:RightsImpact ;
    skos:definition "The gradual weakening or reduction of the scope and protection of rights"@en ;
    skos:inScheme risk:risk-taxonomy-classes ;
    skos:prefLabel "Rights Eroded"@en ;
    skos:scopeNote "Erosion of rights typically only applies to passive rights which always apply, since for active rights the exercise of that right is what enables it. An active right can be eroded over time it is limited consistently and increasingly such that the scope of the right is reduced over time. Though specified as a plural i.e. 'rights', this concept can be applied to a singular right"@en .

risk:RightsExercisePrevented a rdfs:Class,
        skos:Concept,
        dpv:RiskConcept,
        risk:PotentialConsequence,
        risk:PotentialImpact,
        risk:PotentialRisk ;
    dct:contributor _:person-georg-p-krog,
        _:person-harshvardhan-j-pandit ;
    dct:created "2022-08-18"^^xsd:date ;
    dct:modified "2024-08-16"^^xsd:date ;
    rdfs:isDefinedBy risk: ;
    sw:term_status "accepted"@en ;
    skos:broader risk:RightsImpact ;
    skos:definition "Actions or measures that prevent an individual or group from exercising their legal rights."@en ;
    skos:inScheme risk:risk-taxonomy-classes ;
    skos:prefLabel "Rights Exercise Prevented"@en ;
    skos:scopeNote "This concept was called \"PreventExercisingOfRights\" in DPV 2.0. Violation of a right is a bar for actionable actions by an authority. Other impacts on right may be found to construe a violation of the right, but that is not necessarily always the case i.e. not all impacts are violations of a right. Though specified as a plural i.e. 'rights', this concept can be applied to a singular right"@en .

risk:RightsImpact a rdfs:Class,
        skos:Concept,
        dpv:RiskConcept,
        risk:PotentialConsequence,
        risk:PotentialImpact,
        risk:PotentialRisk ;
    dct:contributor _:person-harshvardhan-j-pandit ;
    dct:created "2022-08-17"^^xsd:date ;
    dct:modified "2024-08-16"^^xsd:date ;
    dct:source _:b15886bc6e88dcdb258fe59ded7be3abf ;
    vann:example dex:E0088 ;
    rdfs:isDefinedBy risk: ;
    sw:term_status "accepted"@en ;
    skos:broader risk:SocietalRiskConcept ;
    skos:definition "Concept representing Impact to Rights"@en ;
    skos:inScheme risk:risk-taxonomy-classes ;
    skos:prefLabel "Rights Impact"@en ;
    skos:scopeNote "This concept was called \"ImpactToRights\" in DPV 2.0. Though specified as a plural i.e. 'rights', this concept can be applied to a singular right"@en .

risk:RightsLimited a rdfs:Class,
        skos:Concept,
        dpv:RiskConcept,
        risk:PotentialConsequence,
        risk:PotentialImpact,
        risk:PotentialRisk ;
    dct:contributor _:person-georg-p-krog,
        _:person-harshvardhan-j-pandit ;
    dct:created "2022-08-18"^^xsd:date ;
    dct:modified "2024-08-16"^^xsd:date ;
    rdfs:isDefinedBy risk: ;
    sw:term_status "accepted"@en ;
    skos:broader risk:RightsImpact ;
    skos:definition "A limitation or restrictions on the scope or exercise of rights"@en ;
    skos:inScheme risk:risk-taxonomy-classes ;
    skos:prefLabel "Rights Limited"@en ;
    skos:scopeNote "This concept was called \"LimitationOfRights\" in DPV 2.0. The limitation refers to the applicability and scope of the right, and not in the ability to exercise that right. Limitation is therefore fulfilment of the right and its obligations - but for a scope other than what was intended or expected. Though specified as a plural i.e. 'rights', this concept can be applied to a singular right"@en .

risk:RightsObstructed a rdfs:Class,
        skos:Concept,
        dpv:RiskConcept,
        risk:PotentialConsequence,
        risk:PotentialImpact,
        risk:PotentialRisk ;
    dct:created "2024-12-17"^^xsd:date ;
    rdfs:isDefinedBy risk: ;
    sw:term_status "accepted"@en ;
    skos:broader risk:RightsImpact ;
    skos:definition "Interference with or blocking of the exercise of rights"@en ;
    skos:inScheme risk:risk-taxonomy-classes ;
    skos:prefLabel "Rights Obstructed"@en ;
    skos:scopeNote "In obstruction, the right is not denied, limited, or unfulfilled - but the requirements to enable exercise of the rights are increased to the point of discouraging or obstructing the exercise of that right. Though specified as a plural i.e. 'rights', this concept can be applied to a singular right"@en .

risk:RightsUnfulfilled a rdfs:Class,
        skos:Concept,
        dpv:RiskConcept,
        risk:PotentialConsequence,
        risk:PotentialImpact,
        risk:PotentialRisk ;
    dct:created "2024-12-17"^^xsd:date ;
    rdfs:isDefinedBy risk: ;
    sw:term_status "accepted"@en ;
    skos:broader risk:RightsImpact ;
    skos:definition "Failure to meet or complete the fulfilment of rights"@en ;
    skos:inScheme risk:risk-taxonomy-classes ;
    skos:prefLabel "Rights Unfulfilled"@en ;
    skos:scopeNote "Here unfulfilment refers to non-completion of the right's obligations and processes. Though specified as a plural i.e. 'rights', this concept can be applied to a singular right"@en .

risk:RightsViolated a rdfs:Class,
        skos:Concept,
        dpv:RiskConcept,
        risk:PotentialConsequence,
        risk:PotentialImpact,
        risk:PotentialRisk ;
    dct:contributor _:person-georg-p-krog,
        _:person-harshvardhan-j-pandit ;
    dct:created "2022-08-18"^^xsd:date ;
    dct:modified "2024-08-16"^^xsd:date ;
    vann:example dex:E0088 ;
    rdfs:isDefinedBy risk: ;
    sw:term_status "accepted"@en ;
    skos:broader risk:RightsImpact ;
    skos:definition "The infringement or breach of rights in a manner that constitutes a 'violation' of those rights"@en ;
    skos:inScheme risk:risk-taxonomy-classes ;
    skos:prefLabel "Rights Violated"@en ;
    skos:scopeNote "This concept was called \"ViolationOfRights\" in DPV 2.0. Though specified as a plural i.e. 'rights', this concept can be applied to a singular right"@en .

risk:RiskAcceptance a rdfs:Class,
        skos:Concept ;
    dct:created "2024-12-01"^^xsd:date ;
    rdfs:isDefinedBy risk: ;
    rdfs:subClassOf risk:RiskManagement ;
    sw:term_status "accepted"@en ;
    skos:broader risk:RiskManagement ;
    skos:definition "Entity decision to accept or enable a particular risk"@en ;
    skos:inScheme risk:risk-management-classes ;
    skos:prefLabel "Risk Acceptance"@en .

risk:RiskAnalysis a rdfs:Class,
        skos:Concept ;
    dct:contributor _:person-harshvardhan-j-pandit ;
    dct:created "2022-08-18"^^xsd:date ;
    dct:source _:b3f250dcd774fd0efbd1543bc5def1d0b ;
    rdfs:isDefinedBy risk: ;
    rdfs:subClassOf risk:RiskAssessment ;
    sw:term_status "accepted"@en ;
    skos:broader risk:RiskAssessment ;
    skos:definition "A technique or method used to analyse and identify risk levels, sources, likelihoods, severities, and other necessary information required to conduct risk management procedures"@en ;
    skos:inScheme risk:risk-management-classes ;
    skos:prefLabel "Risk Analysis"@en .

risk:RiskAssessment a rdfs:Class,
        skos:Concept ;
    dct:created "2024-02-14"^^xsd:date ;
    dct:source "ISO 31073:2022 Risk management vocabulary"@en ;
    rdfs:isDefinedBy risk: ;
    rdfs:subClassOf risk:RiskManagement ;
    sw:term_status "accepted"@en ;
    skos:broader risk:RiskManagement ;
    skos:definition "Assessment of risk involving its identification, analysis, and evaluation"@en ;
    skos:inScheme risk:risk-management-classes ;
    skos:prefLabel "Risk Assessment"@en .

risk:RiskControl a rdfs:Class,
        skos:Concept ;
    dct:created "2024-05-19"^^xsd:date ;
    dct:modified "2025-01-06"^^xsd:date ;
    vann:example dex:E0071,
        dex:E0086 ;
    rdfs:isDefinedBy risk: ;
    rdfs:subClassOf dpv:RiskMitigationMeasure ;
    sw:term_status "accepted"@en ;
    skos:broader dpv:RiskMitigationMeasure ;
    skos:definition "Control that modifies risk"@en ;
    skos:inScheme risk:risk-controls-classes ;
    skos:prefLabel "Risk Control"@en .

risk:RiskCriteria a rdfs:Class,
        skos:Concept ;
    dct:created "2024-12-01"^^xsd:date ;
    rdfs:isDefinedBy risk: ;
    rdfs:subClassOf risk:RiskManagement ;
    sw:term_status "accepted"@en ;
    skos:broader risk:RiskManagement ;
    skos:definition "Criteria for determining or evaluating significance of risk"@en ;
    skos:inScheme risk:risk-management-classes ;
    skos:prefLabel "Risk Criteria"@en .

risk:RiskEvaluation a rdfs:Class,
        skos:Concept ;
    dct:created "2024-12-01"^^xsd:date ;
    rdfs:isDefinedBy risk: ;
    rdfs:subClassOf risk:RiskAssessment ;
    sw:term_status "accepted"@en ;
    skos:broader risk:RiskAssessment ;
    skos:definition "Process determining acceptability or tolerance of risk by comparing risk analysis outcomes against risk criteria"@en ;
    skos:inScheme risk:risk-management-classes ;
    skos:prefLabel "Risk Evaluation"@en .

risk:RiskIdentification a rdfs:Class,
        skos:Concept ;
    dct:created "2024-12-01"^^xsd:date ;
    rdfs:isDefinedBy risk: ;
    rdfs:subClassOf risk:RiskAssessment ;
    sw:term_status "accepted"@en ;
    skos:broader risk:RiskAssessment ;
    skos:definition "Identification of risks involving identification of risk sources, potential incidents, their causes, and their potential consequences"@en ;
    skos:inScheme risk:risk-management-classes ;
    skos:prefLabel "Risk Identification"@en .

risk:RiskManagement a rdfs:Class,
        skos:Concept ;
    dct:created "2024-06-12"^^xsd:date ;
    dct:source "ISO 31073:2022 Risk management vocabulary"@en ;
    rdfs:isDefinedBy risk: ;
    rdfs:subClassOf rdfs:Class ;
    sw:term_status "accepted"@en ;
    skos:definition "Systematic application of management policies, procedures, and practices for communicating, consulting, establishing context, and identifying, analysing, evaluating, treating, monitoring and reviewing risk. ISO 31000 definition: coordinated activities to direct and control an organization with regard to risk"@en ;
    skos:inScheme risk:risk-management-classes ;
    skos:prefLabel "Risk Management"@en .

risk:RiskMatrix a rdfs:Class,
        skos:Concept ;
    dct:contributor _:person-harshvardhan-j-pandit ;
    dct:created "2024-02-14"^^xsd:date ;
    dct:source _:b3f250dcd774fd0efbd1543bc5def1d0b ;
    rdfs:isDefinedBy risk: ;
    rdfs:subClassOf risk:RiskAnalysis ;
    sw:term_status "accepted"@en ;
    skos:broader risk:RiskAnalysis ;
    skos:definition "Compares individual risks by selecting a consequence/ likelihood pair and displaying them on a matrix with consequence on one axis and likelihood on the other."@en ;
    skos:inScheme risk:risk-management-classes ;
    skos:prefLabel "Risk Matrix"@en .

risk:RiskMatrix3x3 a rdfs:Class,
        skos:Concept,
        risk:RiskAnalysis ;
    dct:contributor _:person-harshvardhan-j-pandit ;
    dct:created "2022-08-17"^^xsd:date ;
    rdfs:isDefinedBy risk: ;
    sw:term_status "accepted"@en ;
    skos:broader risk:RiskMatrix ;
    skos:definition "A Risk Matrix with 3 Likelihood, 3 Severity, and 3 Risk Level types"@en ;
    skos:inScheme risk:risk-matrix-classes ;
    skos:prefLabel "Risk Matrix 3x3"@en .

risk:RiskMatrix5x5 a rdfs:Class,
        skos:Concept,
        risk:RiskAnalysis ;
    dct:contributor _:person-harshvardhan-j-pandit ;
    dct:created "2022-08-17"^^xsd:date ;
    rdfs:isDefinedBy risk: ;
    sw:term_status "accepted"@en ;
    skos:broader risk:RiskMatrix ;
    skos:definition "A Risk Matrix with 5 Likelihood, 5 Severity, and 5 Risk Level types"@en ;
    skos:inScheme risk:risk-matrix-classes ;
    skos:prefLabel "Risk Matrix 5x5"@en .

risk:RiskMatrix7x7 a rdfs:Class,
        skos:Concept,
        risk:RiskAnalysis ;
    dct:contributor _:person-harshvardhan-j-pandit ;
    dct:created "2022-08-17"^^xsd:date ;
    rdfs:isDefinedBy risk: ;
    sw:term_status "accepted"@en ;
    skos:broader risk:RiskMatrix ;
    skos:definition "A Risk Matrix with 7 Likelihood, 7 Severity, and 7 Risk Level types"@en ;
    skos:inScheme risk:risk-matrix-classes ;
    skos:prefLabel "Risk Matrix 7x7"@en .

risk:RiskOwner a rdfs:Class,
        skos:Concept ;
    dct:created "2024-12-01"^^xsd:date ;
    rdfs:isDefinedBy risk: ;
    rdfs:subClassOf risk:RiskManagement ;
    sw:term_status "accepted"@en ;
    skos:broader risk:RiskManagement ;
    skos:definition "Entity accountable for managing risk"@en ;
    skos:inScheme risk:risk-management-classes ;
    skos:prefLabel "Risk Owner"@en .

risk:RiskPerception a rdfs:Class,
        skos:Concept ;
    dct:created "2024-12-01"^^xsd:date ;
    rdfs:isDefinedBy risk: ;
    rdfs:subClassOf risk:RiskManagement ;
    sw:term_status "accepted"@en ;
    skos:broader risk:RiskManagement ;
    skos:definition "Perception or view on risk"@en ;
    skos:inScheme risk:risk-management-classes ;
    skos:prefLabel "Risk Perception"@en .

risk:RiskSource a rdfs:Class,
        skos:Concept ;
    dct:created "2024-02-14"^^xsd:date ;
    dct:modified "2024-08-16"^^xsd:date ;
    rdfs:isDefinedBy risk: ;
    rdfs:subClassOf risk:RiskIdentification ;
    sw:term_status "accepted"@en ;
    skos:broader risk:RiskIdentification ;
    skos:definition "The 'cause' or 'source', which by itself or with another source has the potential to give rise to risk"@en ;
    skos:inScheme risk:risk-management-classes ;
    skos:prefLabel "Risk Source"@en .

risk:RiskTreatment a rdfs:Class,
        skos:Concept ;
    dct:created "2024-12-01"^^xsd:date ;
    rdfs:isDefinedBy risk: ;
    rdfs:subClassOf risk:RiskManagement ;
    sw:term_status "accepted"@en ;
    skos:broader risk:RiskManagement ;
    skos:definition "Process by which risk is modified and mitigated"@en ;
    skos:inScheme risk:risk-management-classes ;
    skos:prefLabel "Risk Treatment"@en .

risk:RobustnessDegraded a rdfs:Class,
        skos:Concept,
        dpv:RiskConcept,
        risk:PotentialConsequence,
        risk:PotentialRisk,
        risk:PotentialRiskSource ;
    dct:contributor _:person-delaram-golpayegani,
        _:person-harshvardhan-j-pandit ;
    dct:created "2024-12-01"^^xsd:date ;
    rdfs:isDefinedBy risk: ;
    sw:term_status "accepted"@en ;
    skos:broader risk:QualityDegraded,
        risk:RobustnessRisk ;
    skos:definition "Concepts representing risks and issues where Robustness is Degraded"@en ;
    skos:inScheme risk:risk-taxonomy-classes ;
    skos:prefLabel "Robustness Degraded"@en .

risk:RobustnessInconsistent a rdfs:Class,
        skos:Concept,
        dpv:RiskConcept,
        risk:PotentialConsequence,
        risk:PotentialRisk,
        risk:PotentialRiskSource ;
    dct:contributor _:person-harshvardhan-j-pandit ;
    dct:created "2024-12-01"^^xsd:date ;
    rdfs:isDefinedBy risk: ;
    sw:term_status "accepted"@en ;
    skos:broader risk:QualityInconsistent,
        risk:RobustnessRisk ;
    skos:definition "Concepts representing risks and issues where Robustness is Inconsistent"@en ;
    skos:inScheme risk:risk-taxonomy-classes ;
    skos:prefLabel "Robustness Inconsistent"@en .

risk:RobustnessInsufficient a rdfs:Class,
        skos:Concept,
        dpv:RiskConcept,
        risk:PotentialConsequence,
        risk:PotentialRisk,
        risk:PotentialRiskSource ;
    dct:contributor _:person-delaram-golpayegani,
        _:person-harshvardhan-j-pandit ;
    dct:created "2024-12-01"^^xsd:date ;
    rdfs:isDefinedBy risk: ;
    sw:term_status "accepted"@en ;
    skos:broader risk:QualityInsufficient,
        risk:RobustnessRisk ;
    skos:definition "Concepts representing risks and issues where Robustness is Insufficient"@en ;
    skos:inScheme risk:risk-taxonomy-classes ;
    skos:prefLabel "Robustness Insufficient"@en .

risk:RobustnessRisk a rdfs:Class,
        skos:Concept,
        dpv:RiskConcept,
        risk:PotentialConsequence,
        risk:PotentialRisk,
        risk:PotentialRiskSource ;
    dct:contributor _:person-harshvardhan-j-pandit ;
    dct:created "2024-12-01"^^xsd:date ;
    rdfs:isDefinedBy risk: ;
    sw:term_status "accepted"@en ;
    skos:broader risk:QualityRisk ;
    skos:definition "Concepts representing risks and issues where Robustness is Risk"@en ;
    skos:inScheme risk:risk-taxonomy-classes ;
    skos:prefLabel "Robustness Risk"@en .

risk:RobustnessUnknown a rdfs:Class,
        skos:Concept,
        dpv:RiskConcept,
        risk:PotentialConsequence,
        risk:PotentialRisk,
        risk:PotentialRiskSource ;
    dct:contributor _:person-harshvardhan-j-pandit ;
    dct:created "2024-12-01"^^xsd:date ;
    rdfs:isDefinedBy risk: ;
    sw:term_status "accepted"@en ;
    skos:broader risk:QualityUnknown,
        risk:RobustnessRisk ;
    skos:definition "Concepts representing risks and issues where Robustness is Unknown"@en ;
    skos:inScheme risk:risk-taxonomy-classes ;
    skos:prefLabel "Robustness Unknown"@en .

risk:RobustnessUnverified a rdfs:Class,
        skos:Concept,
        dpv:RiskConcept,
        risk:PotentialConsequence,
        risk:PotentialRisk,
        risk:PotentialRiskSource ;
    dct:contributor _:person-harshvardhan-j-pandit ;
    dct:created "2024-12-01"^^xsd:date ;
    rdfs:isDefinedBy risk: ;
    sw:term_status "accepted"@en ;
    skos:broader risk:QualityUnverified,
        risk:RobustnessRisk ;
    skos:definition "Concepts representing risks and issues where Robustness is Unverified"@en ;
    skos:inScheme risk:risk-taxonomy-classes ;
    skos:prefLabel "Robustness Unverified"@en .

risk:RuleBasedSystemDesign a rdfs:Class,
        skos:Concept,
        dpv:RiskConcept,
        risk:PotentialConsequence,
        risk:PotentialRisk,
        risk:PotentialRiskSource ;
    dct:contributor _:person-daniel-doherty,
        _:person-delaram-golpayegani,
        _:person-harshvardhan-j-pandit ;
    dct:created "2024-09-13"^^xsd:date ;
    dct:source "ISO/IEC 24027:2021"@en ;
    rdfs:isDefinedBy risk: ;
    sw:term_status "accepted"@en ;
    skos:broader risk:CognitiveBias ;
    skos:definition "Bias that occurs due to developer experience and expert advice having a significant influence on rule-based system design"@en ;
    skos:inScheme risk:risk-taxonomy-classes ;
    skos:prefLabel "Rule-Based System Design"@en ;
    skos:scopeNote "Rule based system design also potentially introduces various forms of human cognitive bias"@en .

risk:Sabotage a rdfs:Class,
        skos:Concept,
        dpv:RiskConcept,
        risk:AvailabilityConcept,
        risk:IntegrityConcept,
        risk:PotentialConsequence,
        risk:PotentialRisk,
        risk:PotentialRiskSource ;
    dct:contributor _:person-harshvardhan-j-pandit ;
    dct:created "2022-08-17"^^xsd:date ;
    dct:modified "2026-02-09"^^xsd:date ;
    dct:source _:b7191aa21b975cb14bbce32aa3ba9c7eb ;
    rdfs:isDefinedBy risk: ;
    sw:term_status "modified"@en ;
    skos:broader risk:Deception ;
    skos:definition "Concept representing Sabotage"@en ;
    skos:inScheme risk:risk-taxonomy-classes ;
    skos:prefLabel "Sabotage"@en .

risk:Safety a rdfs:Class,
        skos:Concept,
        dpv:RiskConcept,
        risk:PotentialConsequence,
        risk:PotentialImpact,
        risk:PotentialRisk ;
    dct:contributor _:person-harshvardhan-j-pandit ;
    dct:created "2024-12-01"^^xsd:date ;
    rdfs:isDefinedBy risk: ;
    sw:term_status "accepted"@en ;
    skos:broader risk:HealthSafety ;
    skos:definition "Concept representing safety of individual(s), or group(s), or society at large"@en ;
    skos:inScheme risk:risk-taxonomy-classes ;
    skos:prefLabel "Safety"@en .

risk:SamplingBias a rdfs:Class,
        skos:Concept,
        dpv:RiskConcept,
        risk:PotentialConsequence,
        risk:PotentialRisk,
        risk:PotentialRiskSource ;
    dct:contributor _:person-daniel-doherty,
        _:person-delaram-golpayegani,
        _:person-harshvardhan-j-pandit ;
    dct:created "2024-09-13"^^xsd:date ;
    dct:source "ISO/IEC 24027:2021"@en ;
    rdfs:isDefinedBy risk: ;
    sw:term_status "accepted"@en ;
    skos:broader risk:SelectionBias ;
    skos:definition "Bias that occurs when data records are not collected randomly from the intended population"@en ;
    skos:inScheme risk:risk-taxonomy-classes ;
    skos:prefLabel "Sampling Bias"@en .

risk:Scam a rdfs:Class,
        skos:Concept,
        dpv:RiskConcept,
        risk:ConfidentialityConcept,
        risk:PotentialConsequence,
        risk:PotentialRisk,
        risk:PotentialRiskSource ;
    dct:contributor _:person-harshvardhan-j-pandit ;
    dct:created "2022-08-17"^^xsd:date ;
    dct:modified "2026-02-09"^^xsd:date ;
    dct:source _:b15886bc6e88dcdb258fe59ded7be3abf ;
    rdfs:isDefinedBy risk: ;
    sw:term_status "modified"@en ;
    skos:broader risk:Deception ;
    skos:definition "Concept representing Scam"@en ;
    skos:inScheme risk:risk-taxonomy-classes ;
    skos:prefLabel "Scam"@en .

risk:SecurityAttack a rdfs:Class,
        skos:Concept,
        dpv:RiskConcept,
        risk:AvailabilityConcept,
        risk:ConfidentialityConcept,
        risk:IntegrityConcept,
        risk:PotentialRisk,
        risk:PotentialRiskSource ;
    dct:created "2024-12-17"^^xsd:date ;
    rdfs:isDefinedBy risk: ;
    sw:term_status "accepted"@en ;
    skos:broader risk:ExternalSecurityThreat ;
    skos:definition "Concept representing an attack on security with the aim of undermining it"@en ;
    skos:inScheme risk:risk-taxonomy-classes ;
    skos:prefLabel "Security Attack"@en .

risk:SecurityBreach a rdfs:Class,
        skos:Concept,
        dpv:RiskConcept,
        risk:AvailabilityConcept,
        risk:ConfidentialityConcept,
        risk:IntegrityConcept,
        risk:PotentialConsequence,
        risk:PotentialRisk,
        risk:PotentialRiskSource ;
    dct:contributor _:person-harshvardhan-j-pandit ;
    dct:created "2022-08-17"^^xsd:date ;
    dct:modified "2024-08-16"^^xsd:date ;
    dct:source _:b15886bc6e88dcdb258fe59ded7be3abf ;
    rdfs:isDefinedBy risk: ;
    sw:term_status "accepted"@en ;
    skos:broader risk:OperationalSecurityRisk ;
    skos:definition "Concept representing Security Breach"@en ;
    skos:inScheme risk:risk-taxonomy-classes ;
    skos:prefLabel "Security Breach"@en .

risk:SecurityQualityDegraded a rdfs:Class,
        skos:Concept,
        dpv:RiskConcept,
        risk:PotentialConsequence,
        risk:PotentialRisk,
        risk:PotentialRiskSource ;
    dct:contributor _:person-delaram-golpayegani,
        _:person-harshvardhan-j-pandit ;
    dct:created "2024-12-01"^^xsd:date ;
    rdfs:isDefinedBy risk: ;
    sw:term_status "accepted"@en ;
    skos:broader risk:QualityDegraded,
        risk:SecurityQualityRisk ;
    skos:definition "Concepts representing risks and issues where Quality of Security is Degraded"@en ;
    skos:inScheme risk:risk-taxonomy-classes ;
    skos:prefLabel "Security Quality Degraded"@en .

risk:SecurityQualityInconsistent a rdfs:Class,
        skos:Concept,
        dpv:RiskConcept,
        risk:PotentialConsequence,
        risk:PotentialRisk,
        risk:PotentialRiskSource ;
    dct:contributor _:person-harshvardhan-j-pandit ;
    dct:created "2024-12-01"^^xsd:date ;
    rdfs:isDefinedBy risk: ;
    sw:term_status "accepted"@en ;
    skos:broader risk:QualityInconsistent,
        risk:SecurityQualityRisk ;
    skos:definition "Concepts representing risks and issues where Quality of Security is Inconsistent"@en ;
    skos:inScheme risk:risk-taxonomy-classes ;
    skos:prefLabel "Security Quality Inconsistent"@en .

risk:SecurityQualityInsufficient a rdfs:Class,
        skos:Concept,
        dpv:RiskConcept,
        risk:PotentialConsequence,
        risk:PotentialRisk,
        risk:PotentialRiskSource ;
    dct:contributor _:person-delaram-golpayegani,
        _:person-harshvardhan-j-pandit ;
    dct:created "2024-12-01"^^xsd:date ;
    rdfs:isDefinedBy risk: ;
    sw:term_status "accepted"@en ;
    skos:broader risk:QualityInsufficient,
        risk:SecurityQualityRisk ;
    skos:definition "Concepts representing risks and issues where Quality of Security is Insufficient"@en ;
    skos:inScheme risk:risk-taxonomy-classes ;
    skos:prefLabel "Security Quality Insufficient"@en .

risk:SecurityQualityRisk a rdfs:Class,
        skos:Concept,
        dpv:RiskConcept,
        risk:PotentialConsequence,
        risk:PotentialRisk,
        risk:PotentialRiskSource ;
    dct:contributor _:person-harshvardhan-j-pandit ;
    dct:created "2024-12-01"^^xsd:date ;
    rdfs:isDefinedBy risk: ;
    sw:term_status "accepted"@en ;
    skos:broader risk:QualityRisk ;
    skos:definition "Concepts representing risks and issues where Quality of Security is Risk"@en ;
    skos:inScheme risk:risk-taxonomy-classes ;
    skos:prefLabel "Security Quality Risk"@en .

risk:SecurityQualityUnknown a rdfs:Class,
        skos:Concept,
        dpv:RiskConcept,
        risk:PotentialConsequence,
        risk:PotentialRisk,
        risk:PotentialRiskSource ;
    dct:contributor _:person-harshvardhan-j-pandit ;
    dct:created "2024-12-01"^^xsd:date ;
    rdfs:isDefinedBy risk: ;
    sw:term_status "accepted"@en ;
    skos:broader risk:QualityUnknown,
        risk:SecurityQualityRisk ;
    skos:definition "Concepts representing risks and issues where Quality of Security is Unknown"@en ;
    skos:inScheme risk:risk-taxonomy-classes ;
    skos:prefLabel "Security Quality Unknown"@en .

risk:SecurityQualityUnverified a rdfs:Class,
        skos:Concept,
        dpv:RiskConcept,
        risk:PotentialConsequence,
        risk:PotentialRisk,
        risk:PotentialRiskSource ;
    dct:contributor _:person-harshvardhan-j-pandit ;
    dct:created "2024-12-01"^^xsd:date ;
    rdfs:isDefinedBy risk: ;
    sw:term_status "accepted"@en ;
    skos:broader risk:QualityUnverified,
        risk:SecurityQualityRisk ;
    skos:definition "Concepts representing risks and issues where Quality of Security is Unverified"@en ;
    skos:inScheme risk:risk-taxonomy-classes ;
    skos:prefLabel "Security Quality Unverified"@en .

risk:SelectionBias a rdfs:Class,
        skos:Concept,
        dpv:RiskConcept,
        risk:PotentialConsequence,
        risk:PotentialRisk,
        risk:PotentialRiskSource ;
    dct:contributor _:person-daniel-doherty,
        _:person-delaram-golpayegani,
        _:person-harshvardhan-j-pandit ;
    dct:created "2024-09-13"^^xsd:date ;
    dct:source "ISO/IEC 24027:2021"@en ;
    rdfs:isDefinedBy risk: ;
    sw:term_status "accepted"@en ;
    skos:broader risk:StatisticalBias ;
    skos:definition "Bias that occurs when a dataset's samples are chosen in a way that is not reflective of their real-world distribution"@en ;
    skos:inScheme risk:risk-taxonomy-classes ;
    skos:prefLabel "Selection Bias"@en .

risk:ServiceAlternativeOffered a rdfs:Class,
        skos:Concept,
        dpv:RiskConcept,
        risk:PotentialConsequence,
        risk:PotentialImpact,
        risk:PotentialRisk ;
    dct:created "2024-10-21"^^xsd:date ;
    rdfs:isDefinedBy risk: ;
    sw:term_status "accepted"@en ;
    skos:broader risk:ServiceRelatedConsequence ;
    skos:definition "Concept representing service alternative offered"@en ;
    skos:inScheme risk:risk-taxonomy-classes ;
    skos:prefLabel "Service Alternative Offered"@en .

risk:ServiceCostIncreased a rdfs:Class,
        skos:Concept,
        dpv:RiskConcept,
        risk:PotentialConsequence,
        risk:PotentialImpact,
        risk:PotentialRisk ;
    dct:created "2024-10-21"^^xsd:date ;
    rdfs:isDefinedBy risk: ;
    sw:term_status "accepted"@en ;
    skos:broader risk:ServiceRelatedConsequence ;
    skos:definition "Concept representing service cost increased"@en ;
    skos:inScheme risk:risk-taxonomy-classes ;
    skos:prefLabel "Service Cost Increased"@en .

risk:ServiceDenied a rdfs:Class,
        skos:Concept,
        dpv:RiskConcept,
        risk:PotentialConsequence,
        risk:PotentialImpact,
        risk:PotentialRisk ;
    dct:created "2024-10-21"^^xsd:date ;
    rdfs:isDefinedBy risk: ;
    sw:term_status "accepted"@en ;
    skos:broader risk:ServiceRelatedConsequence ;
    skos:definition "Concept representing service denied"@en ;
    skos:inScheme risk:risk-taxonomy-classes ;
    skos:prefLabel "Service Denied"@en .

risk:ServiceLimited a rdfs:Class,
        skos:Concept,
        dpv:RiskConcept,
        risk:PotentialConsequence,
        risk:PotentialImpact,
        risk:PotentialRisk ;
    dct:created "2024-10-21"^^xsd:date ;
    rdfs:isDefinedBy risk: ;
    sw:term_status "accepted"@en ;
    skos:broader risk:ServiceRelatedConsequence ;
    skos:definition "Concept representing service limited"@en ;
    skos:inScheme risk:risk-taxonomy-classes ;
    skos:prefLabel "Service Limited"@en .

risk:ServiceNotProvided a rdfs:Class,
        skos:Concept,
        dpv:RiskConcept,
        risk:PotentialConsequence,
        risk:PotentialImpact,
        risk:PotentialRisk ;
    dct:created "2024-10-21"^^xsd:date ;
    rdfs:isDefinedBy risk: ;
    sw:term_status "accepted"@en ;
    skos:broader risk:ServiceRelatedConsequence ;
    skos:definition "Concept representing service not provided"@en ;
    skos:inScheme risk:risk-taxonomy-classes ;
    skos:prefLabel "Service Not Provided"@en .

risk:ServicePartiallyProvided a rdfs:Class,
        skos:Concept,
        dpv:RiskConcept,
        risk:PotentialConsequence,
        risk:PotentialImpact,
        risk:PotentialRisk ;
    dct:created "2024-10-21"^^xsd:date ;
    rdfs:isDefinedBy risk: ;
    sw:term_status "accepted"@en ;
    skos:broader risk:ServiceRelatedConsequence ;
    skos:definition "Concept representing service partially provided"@en ;
    skos:inScheme risk:risk-taxonomy-classes ;
    skos:prefLabel "Service Partially Provided"@en .

risk:ServiceProvided a rdfs:Class,
        skos:Concept,
        dpv:RiskConcept,
        risk:PotentialConsequence,
        risk:PotentialImpact,
        risk:PotentialRisk ;
    dct:created "2024-10-21"^^xsd:date ;
    rdfs:isDefinedBy risk: ;
    sw:term_status "accepted"@en ;
    skos:broader risk:ServiceRelatedConsequence ;
    skos:definition "Concept representing service provided"@en ;
    skos:inScheme risk:risk-taxonomy-classes ;
    skos:prefLabel "Service Provided"@en .

risk:ServiceProvisionDelayed a rdfs:Class,
        skos:Concept,
        dpv:RiskConcept,
        risk:PotentialConsequence,
        risk:PotentialImpact,
        risk:PotentialRisk ;
    dct:created "2024-10-21"^^xsd:date ;
    rdfs:isDefinedBy risk: ;
    sw:term_status "accepted"@en ;
    skos:broader risk:ServiceRelatedConsequence ;
    skos:definition "Concept representing service provision delayed"@en ;
    skos:inScheme risk:risk-taxonomy-classes ;
    skos:prefLabel "Service Provision Delayed"@en .

risk:ServiceQualityReduced a rdfs:Class,
        skos:Concept,
        dpv:RiskConcept,
        risk:PotentialConsequence,
        risk:PotentialImpact,
        risk:PotentialRisk ;
    dct:created "2024-10-21"^^xsd:date ;
    rdfs:isDefinedBy risk: ;
    sw:term_status "accepted"@en ;
    skos:broader risk:ServiceRelatedConsequence ;
    skos:definition "Concept representing service quality reduced"@en ;
    skos:inScheme risk:risk-taxonomy-classes ;
    skos:prefLabel "Service Quality Reduced"@en .

risk:ServiceRelatedConsequence a rdfs:Class,
        skos:Concept,
        dpv:RiskConcept,
        risk:PotentialConsequence,
        risk:PotentialImpact,
        risk:PotentialRisk ;
    dct:created "2024-10-21"^^xsd:date ;
    rdfs:isDefinedBy risk: ;
    sw:term_status "accepted"@en ;
    skos:broader risk:OrganisationalRiskConcept ;
    skos:definition "A consequence related to the provision of a service"@en ;
    skos:inScheme risk:risk-taxonomy-classes ;
    skos:prefLabel "Service Related Consequence"@en .

risk:ServiceSecurityReduced a rdfs:Class,
        skos:Concept,
        dpv:RiskConcept,
        risk:PotentialConsequence,
        risk:PotentialImpact,
        risk:PotentialRisk ;
    dct:created "2024-10-21"^^xsd:date ;
    rdfs:isDefinedBy risk: ;
    sw:term_status "accepted"@en ;
    skos:broader risk:ServiceRelatedConsequence ;
    skos:definition "Concept representing service security reduced"@en ;
    skos:inScheme risk:risk-taxonomy-classes ;
    skos:prefLabel "Service Security Reduced"@en .

risk:ServiceTermination a rdfs:Class,
        skos:Concept,
        dpv:RiskConcept,
        risk:PotentialConsequence,
        risk:PotentialImpact,
        risk:PotentialRisk ;
    dct:created "2024-10-21"^^xsd:date ;
    rdfs:isDefinedBy risk: ;
    sw:term_status "accepted"@en ;
    skos:broader risk:ServiceRelatedConsequence ;
    skos:definition "Concept representing service termination"@en ;
    skos:inScheme risk:risk-taxonomy-classes ;
    skos:prefLabel "Service Termination"@en .

risk:SexDiscrimination a rdfs:Class,
        skos:Concept,
        dpv:RiskConcept,
        risk:PotentialConsequence,
        risk:PotentialImpact,
        risk:PotentialRisk ;
    dct:created "2024-09-30"^^xsd:date ;
    rdfs:isDefinedBy risk: ;
    sw:term_status "accepted"@en ;
    skos:broader risk:Sexism ;
    skos:definition "Discrimination based on a person's biological sex"@en ;
    skos:inScheme risk:risk-taxonomy-classes ;
    skos:prefLabel "Sex Discrimination"@en .

risk:Sexism a rdfs:Class,
        skos:Concept,
        dpv:RiskConcept,
        risk:PotentialConsequence,
        risk:PotentialImpact,
        risk:PotentialRisk ;
    dct:created "2024-09-30"^^xsd:date ;
    rdfs:isDefinedBy risk: ;
    sw:term_status "accepted"@en ;
    skos:broader risk:Discrimination ;
    skos:definition "Discrimination based on a person's sex or gender, typically involving unequal treatment or stereotyping"@en ;
    skos:inScheme risk:risk-taxonomy-classes ;
    skos:prefLabel "Sexism"@en .

risk:SexualHarassment a rdfs:Class,
        skos:Concept,
        dpv:RiskConcept,
        risk:PotentialConsequence,
        risk:PotentialImpact,
        risk:PotentialRisk ;
    dct:created "2022-08-17"^^xsd:date ;
    dct:modified "2024-12-01"^^xsd:date ;
    rdfs:isDefinedBy risk: ;
    sw:term_status "modified"@en ;
    skos:broader risk:Harassment ;
    skos:definition "Concept representing sexual harassment of individual(s)"@en ;
    skos:inScheme risk:risk-taxonomy-classes ;
    skos:prefLabel "Sexual Harassment"@en .

risk:SexualOrientationDiscrimination a rdfs:Class,
        skos:Concept,
        dpv:RiskConcept,
        risk:PotentialConsequence,
        risk:PotentialImpact,
        risk:PotentialRisk ;
    dct:created "2024-09-30"^^xsd:date ;
    rdfs:isDefinedBy risk: ;
    sw:term_status "accepted"@en ;
    skos:broader risk:Discrimination ;
    skos:definition "Discrimination based on a person's sexual orientation, typically against those who are not heterosexual"@en ;
    skos:inScheme risk:risk-taxonomy-classes ;
    skos:prefLabel "SexualOrientation Discrimination"@en .

risk:SexualViolence a rdfs:Class,
        skos:Concept,
        dpv:RiskConcept,
        risk:PotentialConsequence,
        risk:PotentialImpact,
        risk:PotentialRisk ;
    dct:contributor _:person-harshvardhan-j-pandit ;
    dct:created "2022-08-17"^^xsd:date ;
    dct:modified "2024-08-16"^^xsd:date ;
    dct:source _:b7191aa21b975cb14bbce32aa3ba9c7eb ;
    rdfs:isDefinedBy risk: ;
    sw:term_status "accepted"@en ;
    skos:broader risk:Harm,
        risk:MentalSafety,
        risk:PhysicalSafety ;
    skos:definition "Concept representing Sexual Violence"@en ;
    skos:inScheme risk:risk-taxonomy-classes ;
    skos:prefLabel "Sexual Violence"@en .

risk:ShareControl a rdfs:Class,
        skos:Concept,
        risk:RiskControl ;
    dct:contributor _:person-harshvardhan-j-pandit ;
    dct:created "2025-01-06"^^xsd:date ;
    rdfs:isDefinedBy risk: ;
    sw:term_status "accepted"@en ;
    skos:broader risk:TransferControl ;
    skos:definition "Control that aims to share or distribute the event (or risk) with another context or entity"@en ;
    skos:inScheme risk:risk-controls-classes ;
    skos:prefLabel "Share Control"@en ;
    skos:scopeNote "Sharing implies a combined responsibility or sharing of effects from an event - which can be between entities or processes (or other contexts). The use of 'event' here broadly refers to any event, which may be a risk event or could also be specific measures being adopted in response to an event. For specifically indicating sharing of risk per typical risk management processes, see risk:ShareRisk"@en .

risk:ShareRisk a rdfs:Class,
        skos:Concept,
        risk:RiskControl ;
    dct:contributor _:person-harshvardhan-j-pandit ;
    dct:created "2024-05-19"^^xsd:date ;
    dct:modified "2025-01-06"^^xsd:date ;
    rdfs:isDefinedBy risk: ;
    sw:term_status "modified"@en ;
    skos:broader risk:ShareControl ;
    skos:definition "Risk Mitigation Measure that shares Risk e.g. amongst stakeholders"@en ;
    skos:inScheme risk:risk-controls-classes ;
    skos:prefLabel "Share Risk"@en .

risk:SimpsonsParadoxBias a rdfs:Class,
        skos:Concept,
        dpv:RiskConcept,
        risk:PotentialConsequence,
        risk:PotentialRisk,
        risk:PotentialRiskSource ;
    dct:contributor _:person-daniel-doherty,
        _:person-delaram-golpayegani,
        _:person-harshvardhan-j-pandit ;
    dct:created "2024-09-13"^^xsd:date ;
    dct:source "ISO/IEC 24027:2021"@en ;
    rdfs:isDefinedBy risk: ;
    sw:term_status "accepted"@en ;
    skos:broader risk:DataBias ;
    skos:definition "Bias that occurs when a trend that is indicated in individual groups of data reverses when the groups of data are combined"@en ;
    skos:inScheme risk:risk-taxonomy-classes ;
    skos:prefLabel "Simpson'S Paradox Bias"@en .

risk:SocialDisadvantage a rdfs:Class,
        skos:Concept,
        dpv:RiskConcept,
        risk:PotentialConsequence,
        risk:PotentialImpact,
        risk:PotentialRisk ;
    dct:contributor _:person-georg-p-krog ;
    dct:created "2022-08-19"^^xsd:date ;
    dct:modified "2024-08-16"^^xsd:date ;
    rdfs:isDefinedBy risk: ;
    sw:term_status "accepted"@en ;
    skos:broader risk:GroupRisk ;
    skos:definition "Concept representing Social Disadvantage"@en ;
    skos:inScheme risk:risk-taxonomy-classes ;
    skos:prefLabel "Social Disadvantage"@en .

risk:SocietalBias a rdfs:Class,
        skos:Concept,
        dpv:RiskConcept,
        risk:PotentialConsequence,
        risk:PotentialRisk,
        risk:PotentialRiskSource ;
    dct:contributor _:person-daniel-doherty,
        _:person-delaram-golpayegani,
        _:person-harshvardhan-j-pandit ;
    dct:created "2024-09-13"^^xsd:date ;
    dct:source "ISO/IEC 24027:2021"@en ;
    rdfs:isDefinedBy risk: ;
    sw:term_status "accepted"@en ;
    skos:broader risk:CognitiveBias ;
    skos:definition "Bias that occurs when similar cognitive bias (conscious or unconscious) is being held by many individuals in society"@en ;
    skos:inScheme risk:risk-taxonomy-classes ;
    skos:prefLabel "Societal Bias"@en .

risk:SocietalHealthSafety a rdfs:Class,
        skos:Concept,
        dpv:RiskConcept,
        risk:PotentialConsequence,
        risk:PotentialImpact,
        risk:PotentialRisk ;
    dct:created "2024-12-17"^^xsd:date ;
    rdfs:isDefinedBy risk: ;
    sw:term_status "accepted"@en ;
    skos:broader risk:GroupRisk ;
    skos:definition "Concept representing health and safety of society at large"@en ;
    skos:inScheme risk:risk-taxonomy-classes ;
    skos:prefLabel "Societal Health & Safety"@en .

risk:SocietalRiskConcept a rdfs:Class,
        skos:Concept,
        dpv:RiskConcept,
        risk:PotentialConsequence,
        risk:PotentialImpact,
        risk:PotentialRisk,
        risk:PotentialRiskSource ;
    dct:created "2024-10-21"^^xsd:date ;
    rdfs:isDefinedBy risk: ;
    sw:term_status "accepted"@en ;
    skos:broader dpv:RiskConcept ;
    skos:definition "Risk concepts, including any potential risk sources, consequences, or impacts, that are societal in nature or relate to a social setting or process"@en ;
    skos:inScheme risk:risk-taxonomy-classes ;
    skos:prefLabel "Societal Risk Concept"@en ;
    skos:scopeNote "Societal in this context includes both individuals and groups in a social context, as well as wider implications for society - such as environmental impacts or economic consequences of inflation that can affect both human and non-human entities as part of the social structure"@en .

risk:SourceControl a rdfs:Class,
        skos:Concept,
        risk:RiskControl ;
    dct:contributor _:person-harshvardhan-j-pandit ;
    dct:created "2024-05-19"^^xsd:date ;
    dct:modified "2025-01-06"^^xsd:date ;
    rdfs:isDefinedBy risk: ;
    sw:term_status "modified"@en ;
    skos:broader risk:RiskControl ;
    skos:definition "Risk control for managing risk sources"@en ;
    skos:inScheme risk:risk-controls-classes ;
    skos:prefLabel "Source Control"@en .

risk:Spoofing a rdfs:Class,
        skos:Concept,
        dpv:RiskConcept,
        risk:ConfidentialityConcept,
        risk:IntegrityConcept,
        risk:PotentialConsequence,
        risk:PotentialRisk,
        risk:PotentialRiskSource ;
    dct:contributor _:person-harshvardhan-j-pandit ;
    dct:created "2022-08-17"^^xsd:date ;
    dct:modified "2026-02-09"^^xsd:date ;
    dct:source _:b15886bc6e88dcdb258fe59ded7be3abf ;
    rdfs:isDefinedBy risk: ;
    sw:term_status "modified"@en ;
    skos:broader risk:Deception ;
    skos:definition "Concept representing Spoofing"@en ;
    skos:inScheme risk:risk-taxonomy-classes ;
    skos:prefLabel "Spoofing"@en .

risk:StaffIncompetence a rdfs:Class,
        skos:Concept,
        dpv:RiskConcept,
        risk:PotentialConsequence,
        risk:PotentialRisk,
        risk:PotentialRiskSource ;
    dct:contributor _:person-delaram-golpayegani,
        _:person-harshvardhan-j-pandit ;
    dct:created "2024-12-01"^^xsd:date ;
    rdfs:isDefinedBy risk: ;
    sw:term_status "accepted"@en ;
    skos:broader risk:OrganisationalManagementRisk ;
    skos:definition "Concept representing incompetence of staff"@en ;
    skos:inScheme risk:risk-taxonomy-classes ;
    skos:prefLabel "Staff Incompetence"@en .

risk:StatisticalBias a rdfs:Class,
        skos:Concept,
        dpv:RiskConcept,
        risk:PotentialConsequence,
        risk:PotentialRisk,
        risk:PotentialRiskSource ;
    dct:contributor _:person-daniel-doherty,
        _:person-delaram-golpayegani,
        _:person-harshvardhan-j-pandit ;
    dct:created "2024-09-13"^^xsd:date ;
    dct:source "ISO 20501:2019"@en ;
    rdfs:isDefinedBy risk: ;
    sw:term_status "accepted"@en ;
    skos:broader risk:DataBias ;
    skos:definition "Bias that occurs as the type of consistent numerical offset in an estimate relative to the true underlying value, inherent to most estimates"@en ;
    skos:inScheme risk:risk-taxonomy-classes ;
    skos:prefLabel "Statistical Bias"@en .

risk:SubstitutionControl a rdfs:Class,
        skos:Concept,
        risk:RiskControl ;
    dct:contributor _:person-delaram-golpayegani,
        _:person-harshvardhan-j-pandit ;
    dct:created "2025-01-06"^^xsd:date ;
    rdfs:isDefinedBy risk: ;
    sw:term_status "accepted"@en ;
    skos:broader risk:AvoidanceControl ;
    skos:definition "Control that substitutes an event with another such that the initial event no longer takes place while the substituted event takes place in place of it"@en ;
    skos:inScheme risk:risk-controls-classes ;
    skos:prefLabel "Substitution Control"@en ;
    skos:scopeNote "Substitution implies that the replacement event is less risky or is more safe than the replaced event, which is distinct from elimination where no event occurs and thus there is an elimination of risk entirely"@en .

risk:SystemFailure a rdfs:Class,
        skos:Concept,
        dpv:RiskConcept,
        risk:AvailabilityConcept,
        risk:PotentialConsequence,
        risk:PotentialRisk,
        risk:PotentialRiskSource ;
    dct:contributor _:person-harshvardhan-j-pandit ;
    dct:created "2022-08-17"^^xsd:date ;
    dct:modified "2024-08-16"^^xsd:date ;
    dct:source _:b89b5ee884952f33d70d4fddc4220b465 ;
    rdfs:isDefinedBy risk: ;
    sw:term_status "accepted"@en ;
    skos:broader risk:OperationalSecurityRisk ;
    skos:definition "Concept representing System Failure"@en ;
    skos:inScheme risk:risk-taxonomy-classes ;
    skos:prefLabel "System Failure"@en ;
    skos:scopeNote "Here system refers to both hardware and software systems"@en .

risk:SystemIntrusion a rdfs:Class,
        skos:Concept,
        dpv:RiskConcept,
        risk:AvailabilityConcept,
        risk:ConfidentialityConcept,
        risk:IntegrityConcept,
        risk:PotentialRisk,
        risk:PotentialRiskSource ;
    dct:contributor _:person-harshvardhan-j-pandit ;
    dct:created "2022-08-17"^^xsd:date ;
    dct:modified "2024-08-16"^^xsd:date ;
    dct:source _:b7191aa21b975cb14bbce32aa3ba9c7eb ;
    rdfs:isDefinedBy risk: ;
    sw:term_status "accepted"@en ;
    skos:broader risk:SecurityAttack ;
    skos:definition "Concept representing System Intrusion"@en ;
    skos:inScheme risk:risk-taxonomy-classes ;
    skos:prefLabel "System Intrusion"@en .

risk:SystemMalfunction a rdfs:Class,
        skos:Concept,
        dpv:RiskConcept,
        risk:AvailabilityConcept,
        risk:PotentialConsequence,
        risk:PotentialRisk,
        risk:PotentialRiskSource ;
    dct:contributor _:person-harshvardhan-j-pandit ;
    dct:created "2022-08-17"^^xsd:date ;
    dct:modified "2024-08-16"^^xsd:date ;
    dct:source _:b15886bc6e88dcdb258fe59ded7be3abf ;
    rdfs:isDefinedBy risk: ;
    sw:term_status "accepted"@en ;
    skos:broader risk:OperationalSecurityRisk ;
    skos:definition "Concept representing System Malfunction"@en ;
    skos:inScheme risk:risk-taxonomy-classes ;
    skos:prefLabel "System Malfunction"@en ;
    skos:scopeNote "Here system refers to both hardware and software systems"@en .

risk:TaskExecutionIncorrect a rdfs:Class,
        skos:Concept,
        dpv:RiskConcept,
        risk:AvailabilityConcept,
        risk:IntegrityConcept,
        risk:PotentialConsequence,
        risk:PotentialRisk,
        risk:PotentialRiskSource ;
    dct:contributor _:person-harshvardhan-j-pandit ;
    dct:created "2024-12-01"^^xsd:date ;
    rdfs:isDefinedBy risk: ;
    sw:term_status "accepted"@en ;
    skos:broader risk:TaskExecutionRisk ;
    skos:definition "Concept representing incorrect execution of task(s)"@en ;
    skos:inScheme risk:risk-taxonomy-classes ;
    skos:prefLabel "Task Execution Incorrect"@en .

risk:TaskExecutionRisk a rdfs:Class,
        skos:Concept,
        dpv:RiskConcept,
        risk:IntegrityConcept,
        risk:PotentialConsequence,
        risk:PotentialRisk,
        risk:PotentialRiskSource ;
    dct:contributor _:person-harshvardhan-j-pandit ;
    dct:created "2024-12-01"^^xsd:date ;
    rdfs:isDefinedBy risk: ;
    sw:term_status "accepted"@en ;
    skos:broader risk:OperationalSecurityRisk ;
    skos:definition "Concept representing risks and issues associated with execution of tasks, operations, activities, and other similar processes"@en ;
    skos:inScheme risk:risk-taxonomy-classes ;
    skos:prefLabel "Task Execution Risk"@en .

risk:TaskOmitted a rdfs:Class,
        skos:Concept,
        dpv:RiskConcept,
        risk:AvailabilityConcept,
        risk:IntegrityConcept,
        risk:PotentialConsequence,
        risk:PotentialRisk,
        risk:PotentialRiskSource ;
    dct:contributor _:person-arthit-suriyawongkul,
        _:person-harshvardhan-j-pandit ;
    dct:created "2024-12-01"^^xsd:date ;
    dct:modified "2025-08-06"^^xsd:date ;
    rdfs:isDefinedBy risk: ;
    sw:term_status "modified"@en ;
    skos:broader risk:TaskExecutionRisk ;
    skos:definition "Concept representing omission of task(s)"@en ;
    skos:inScheme risk:risk-taxonomy-classes ;
    skos:prefLabel "Task Omitted"@en .

risk:TaskTimingIncorrect a rdfs:Class,
        skos:Concept,
        dpv:RiskConcept,
        risk:AvailabilityConcept,
        risk:IntegrityConcept,
        risk:PotentialConsequence,
        risk:PotentialRisk,
        risk:PotentialRiskSource ;
    dct:contributor _:person-harshvardhan-j-pandit ;
    dct:created "2024-12-01"^^xsd:date ;
    rdfs:isDefinedBy risk: ;
    sw:term_status "accepted"@en ;
    skos:broader risk:TaskExecutionRisk ;
    skos:definition "Concept representing incorrect timing for task(s) i.e. the task execution does not occur at the correct time"@en ;
    skos:inScheme risk:risk-taxonomy-classes ;
    skos:prefLabel "Task Timing Incorrect"@en .

risk:TechnicalRiskConcept a rdfs:Class,
        skos:Concept,
        dpv:RiskConcept,
        risk:PotentialConsequence,
        risk:PotentialImpact,
        risk:PotentialRisk,
        risk:PotentialRiskSource ;
    dct:created "2025-01-06"^^xsd:date ;
    rdfs:isDefinedBy risk: ;
    sw:term_status "accepted"@en ;
    skos:broader dpv:RiskConcept ;
    skos:definition "Risk concepts, including any potential risk sources, consequences, or impacts, that are technical in nature or relate to a technical or technological process"@en ;
    skos:inScheme risk:risk-taxonomy-classes ;
    skos:prefLabel "Technical Risk Concept"@en .

risk:TechnologyOverreliance a rdfs:Class,
        skos:Concept,
        dpv:RiskConcept,
        risk:PotentialConsequence,
        risk:PotentialRisk,
        risk:PotentialRiskSource ;
    dct:contributor _:person-delaram-golpayegani,
        _:person-harshvardhan-j-pandit ;
    dct:created "2024-12-01"^^xsd:date ;
    rdfs:isDefinedBy risk: ;
    sw:term_status "accepted"@en ;
    skos:broader risk:OrganisationalManagementRisk ;
    skos:definition "Concept representing the case where an entity, including individuals, have an overreliance on the use of technology"@en ;
    skos:inScheme risk:risk-taxonomy-classes ;
    skos:prefLabel "Technology Overreliance"@en .

risk:Terrorism a rdfs:Class,
        skos:Concept,
        dpv:RiskConcept,
        risk:PotentialConsequence,
        risk:PotentialImpact,
        risk:PotentialRisk ;
    dct:contributor _:person-harshvardhan-j-pandit ;
    dct:created "2022-08-17"^^xsd:date ;
    dct:modified "2024-08-16"^^xsd:date ;
    dct:source _:b15886bc6e88dcdb258fe59ded7be3abf ;
    rdfs:isDefinedBy risk: ;
    sw:term_status "accepted"@en ;
    skos:broader risk:GroupRisk ;
    skos:definition "Concept representing Terrorism"@en ;
    skos:inScheme risk:risk-taxonomy-classes ;
    skos:prefLabel "Terrorism"@en .

risk:Threat a rdfs:Class,
        skos:Concept ;
    dct:created "2024-02-14"^^xsd:date ;
    rdfs:isDefinedBy risk: ;
    rdfs:subClassOf risk:RiskIdentification ;
    sw:term_status "accepted"@en ;
    skos:broader risk:RiskIdentification ;
    skos:definition "Risk source event which causes Risk"@en ;
    skos:inScheme risk:risk-management-classes ;
    skos:prefLabel "Threat"@en .

risk:ThreatSource a rdfs:Class,
        skos:Concept ;
    dct:created "2024-02-14"^^xsd:date ;
    rdfs:isDefinedBy risk: ;
    rdfs:subClassOf risk:RiskIdentification ;
    sw:term_status "accepted"@en ;
    skos:broader risk:RiskIdentification ;
    skos:definition "Source of threat event, including both agent and non-agent sources"@en ;
    skos:inScheme risk:risk-management-classes ;
    skos:prefLabel "Threat Source"@en .

risk:TransferControl a rdfs:Class,
        skos:Concept,
        risk:RiskControl ;
    dct:contributor _:person-harshvardhan-j-pandit ;
    dct:created "2025-01-06"^^xsd:date ;
    rdfs:isDefinedBy risk: ;
    sw:term_status "accepted"@en ;
    skos:broader risk:RiskControl ;
    skos:definition "Control that aims to transfer the event (or risk) to another context or entity"@en ;
    skos:inScheme risk:risk-controls-classes ;
    skos:prefLabel "Transfer Control"@en ;
    skos:scopeNote "Transfer implies moving (physically or logically) the event to another context or entity. While Risk Management methods indicate risk transfer as occurring between entities, this concept is defined more broadly by including 'context or entity' so as to enable modelling cases where the transfer takes place between processes - which may be managed by the same or different entity. Additionally, typical use of 'Transfer' implies a formal mechanism such as an agreement, which is absent from this concept. If only partial responsibility is transferred, such as for a specific measure, then this can be considered as an instance of sharing the risk - for which risk:ShareControl is provided"@en .

risk:TransparencyControl a rdfs:Class,
        skos:Concept,
        risk:RiskControl ;
    dct:contributor _:person-delaram-golpayegani,
        _:person-harshvardhan-j-pandit ;
    dct:created "2025-01-06"^^xsd:date ;
    rdfs:isDefinedBy risk: ;
    sw:term_status "accepted"@en ;
    skos:broader risk:MonitorControl ;
    skos:definition "Control that provides information about an event"@en ;
    skos:inScheme risk:risk-controls-classes ;
    skos:prefLabel "Transparency Control"@en ;
    skos:scopeNote "Transparency refers to the availability of information, whether for the same or different entity in relation to who establishes and operates the control, and where transparency implies having the means to obtain and use information about an event"@en .

risk:Transphobia a rdfs:Class,
        skos:Concept,
        dpv:RiskConcept,
        risk:PotentialConsequence,
        risk:PotentialImpact,
        risk:PotentialRisk ;
    dct:created "2024-09-30"^^xsd:date ;
    rdfs:isDefinedBy risk: ;
    sw:term_status "accepted"@en ;
    skos:broader risk:Sexism ;
    skos:definition "Hostility or prejudice against transgender people or those perceived as not conforming to traditional gender norms"@en ;
    skos:inScheme risk:risk-taxonomy-classes ;
    skos:prefLabel "Transphobia"@en .

risk:TrustLoss a rdfs:Class,
        skos:Concept,
        dpv:RiskConcept,
        risk:PotentialConsequence,
        risk:PotentialImpact,
        risk:PotentialRisk ;
    dct:contributor _:person-harshvardhan-j-pandit ;
    dct:created "2022-08-17"^^xsd:date ;
    dct:modified "2025-08-24"^^xsd:date ;
    dct:source _:b15886bc6e88dcdb258fe59ded7be3abf ;
    rdfs:isDefinedBy risk: ;
    sw:term_status "modified"@en ;
    skos:broader risk:ReputationalRisk ;
    skos:definition "Concept representing Trust Loss"@en ;
    skos:inScheme risk:risk-taxonomy-classes ;
    skos:prefLabel "Trust Loss"@en .

risk:UnauthorisedAccessToPremises a rdfs:Class,
        skos:Concept,
        dpv:RiskConcept,
        risk:AvailabilityConcept,
        risk:ConfidentialityConcept,
        risk:IntegrityConcept,
        risk:PotentialConsequence,
        risk:PotentialRisk,
        risk:PotentialRiskSource ;
    dct:contributor _:person-arthit-suriyawongkul,
        _:person-harshvardhan-j-pandit ;
    dct:created "2022-08-17"^^xsd:date ;
    dct:modified "2025-08-06"^^xsd:date ;
    dct:source _:b15886bc6e88dcdb258fe59ded7be3abf ;
    rdfs:isDefinedBy risk: ;
    sw:term_status "accepted"@en ;
    skos:broader risk:UnauthorisedActivity ;
    skos:definition "Concept representing Unauthorised Access to Premises"@en ;
    skos:inScheme risk:risk-taxonomy-classes ;
    skos:prefLabel "Unauthorised Access to Premises"@en .

risk:UnauthorisedActivity a rdfs:Class,
        skos:Concept,
        dpv:RiskConcept,
        risk:AvailabilityConcept,
        risk:ConfidentialityConcept,
        risk:IntegrityConcept,
        risk:PotentialConsequence,
        risk:PotentialRisk,
        risk:PotentialRiskSource ;
    dct:created "2024-12-17"^^xsd:date ;
    rdfs:isDefinedBy risk: ;
    sw:term_status "accepted"@en ;
    skos:broader risk:ExternalSecurityThreat ;
    skos:definition "Concept representing Unauthorised Activity"@en ;
    skos:inScheme risk:risk-taxonomy-classes ;
    skos:prefLabel "Unauthorised Activity"@en .

risk:UnauthorisedCodeAccess a rdfs:Class,
        skos:Concept,
        dpv:RiskConcept,
        risk:ConfidentialityConcept,
        risk:IntegrityConcept,
        risk:PotentialConsequence,
        risk:PotentialRisk,
        risk:PotentialRiskSource ;
    dct:contributor _:person-harshvardhan-j-pandit ;
    dct:created "2022-08-17"^^xsd:date ;
    dct:modified "2024-08-16"^^xsd:date ;
    dct:source _:bba19dc259a53f0cb59375372938fbb0a ;
    rdfs:isDefinedBy risk: ;
    sw:term_status "accepted"@en ;
    skos:broader risk:UnauthorisedActivity ;
    skos:definition "Concept representing Unauthorised Code Access"@en ;
    skos:inScheme risk:risk-taxonomy-classes ;
    skos:prefLabel "Unauthorised Code Access"@en .

risk:UnauthorisedCodeDisclosure a rdfs:Class,
        skos:Concept,
        dpv:RiskConcept,
        risk:ConfidentialityConcept,
        risk:PotentialConsequence,
        risk:PotentialRisk,
        risk:PotentialRiskSource ;
    dct:contributor _:person-harshvardhan-j-pandit ;
    dct:created "2022-08-17"^^xsd:date ;
    dct:modified "2024-08-16"^^xsd:date ;
    dct:source _:bba19dc259a53f0cb59375372938fbb0a ;
    rdfs:isDefinedBy risk: ;
    sw:term_status "accepted"@en ;
    skos:broader risk:UnauthorisedActivity ;
    skos:definition "Concept representing Unauthorised Code Disclosure"@en ;
    skos:inScheme risk:risk-taxonomy-classes ;
    skos:prefLabel "Unauthorised Code Disclosure"@en .

risk:UnauthorisedCodeModification a rdfs:Class,
        skos:Concept,
        dpv:RiskConcept,
        risk:IntegrityConcept,
        risk:PotentialConsequence,
        risk:PotentialRisk,
        risk:PotentialRiskSource ;
    dct:contributor _:person-harshvardhan-j-pandit ;
    dct:created "2022-08-17"^^xsd:date ;
    dct:modified "2024-08-16"^^xsd:date ;
    dct:source _:bba19dc259a53f0cb59375372938fbb0a ;
    rdfs:isDefinedBy risk: ;
    sw:term_status "accepted"@en ;
    skos:broader risk:UnauthorisedActivity ;
    skos:definition "Concept representing Unauthorised Code Modification"@en ;
    skos:inScheme risk:risk-taxonomy-classes ;
    skos:prefLabel "Unauthorised Code Modification"@en .

risk:UnauthorisedDataAccess a rdfs:Class,
        skos:Concept,
        dpv:RiskConcept,
        risk:ConfidentialityConcept,
        risk:PotentialConsequence,
        risk:PotentialRisk,
        risk:PotentialRiskSource ;
    dct:contributor _:person-harshvardhan-j-pandit ;
    dct:created "2022-08-17"^^xsd:date ;
    dct:modified "2024-08-16"^^xsd:date ;
    dct:source _:b7191aa21b975cb14bbce32aa3ba9c7eb ;
    rdfs:isDefinedBy risk: ;
    sw:term_status "accepted"@en ;
    skos:broader risk:UnauthorisedActivity ;
    skos:definition "Concept representing Unauthorised Data Access"@en ;
    skos:inScheme risk:risk-taxonomy-classes ;
    skos:prefLabel "Unauthorised Data Access"@en .

risk:UnauthorisedDataDisclosure a rdfs:Class,
        skos:Concept,
        dpv:RiskConcept,
        risk:ConfidentialityConcept,
        risk:PotentialConsequence,
        risk:PotentialRisk,
        risk:PotentialRiskSource ;
    dct:contributor _:person-harshvardhan-j-pandit ;
    dct:created "2022-08-17"^^xsd:date ;
    dct:modified "2024-08-16"^^xsd:date ;
    dct:source _:b15886bc6e88dcdb258fe59ded7be3abf ;
    rdfs:isDefinedBy risk: ;
    sw:term_status "accepted"@en ;
    skos:broader risk:UnauthorisedActivity ;
    skos:definition "Concept representing Unauthorised Data Disclosure"@en ;
    skos:inScheme risk:risk-taxonomy-classes ;
    skos:prefLabel "Unauthorised Data Disclosure"@en .

risk:UnauthorisedDataModification a rdfs:Class,
        skos:Concept,
        dpv:RiskConcept,
        risk:IntegrityConcept,
        risk:PotentialConsequence,
        risk:PotentialRisk,
        risk:PotentialRiskSource ;
    dct:contributor _:person-harshvardhan-j-pandit ;
    dct:created "2022-08-17"^^xsd:date ;
    dct:modified "2024-08-16"^^xsd:date ;
    dct:source _:b7191aa21b975cb14bbce32aa3ba9c7eb ;
    rdfs:isDefinedBy risk: ;
    sw:term_status "accepted"@en ;
    skos:broader risk:UnauthorisedActivity ;
    skos:definition "Concept representing Unauthorised Data Modification"@en ;
    skos:inScheme risk:risk-taxonomy-classes ;
    skos:prefLabel "Unauthorised Data Modification"@en .

risk:UnauthorisedInformationDisclosure a rdfs:Class,
        skos:Concept,
        dpv:RiskConcept,
        risk:ConfidentialityConcept,
        risk:PotentialConsequence,
        risk:PotentialRisk,
        risk:PotentialRiskSource ;
    dct:contributor _:person-harshvardhan-j-pandit ;
    dct:created "2022-08-17"^^xsd:date ;
    dct:modified "2024-08-16"^^xsd:date ;
    dct:source _:b7191aa21b975cb14bbce32aa3ba9c7eb ;
    rdfs:isDefinedBy risk: ;
    sw:term_status "accepted"@en ;
    skos:broader risk:UnauthorisedActivity ;
    skos:definition "Concept representing Unauthorised Information Disclosure"@en ;
    skos:inScheme risk:risk-taxonomy-classes ;
    skos:prefLabel "Unauthorised Information Disclosure"@en .

risk:UnauthorisedReidentification a rdfs:Class,
        skos:Concept,
        dpv:RiskConcept,
        risk:ConfidentialityConcept,
        risk:PotentialConsequence,
        risk:PotentialRisk,
        risk:PotentialRiskSource ;
    dct:contributor _:person-georg-p-krog ;
    dct:created "2022-08-19"^^xsd:date ;
    dct:modified "2024-08-16"^^xsd:date ;
    rdfs:isDefinedBy risk: ;
    sw:term_status "accepted"@en ;
    skos:broader risk:UnauthorisedActivity ;
    skos:definition "Concept representing Unauthorised Re-Identification"@en ;
    skos:inScheme risk:risk-taxonomy-classes ;
    skos:prefLabel "Unauthorised Re-Identification"@en .

risk:UnauthorisedResourceUse a rdfs:Class,
        skos:Concept,
        dpv:RiskConcept,
        risk:AvailabilityConcept,
        risk:PotentialConsequence,
        risk:PotentialRisk,
        risk:PotentialRiskSource ;
    dct:contributor _:person-harshvardhan-j-pandit ;
    dct:created "2022-08-17"^^xsd:date ;
    dct:modified "2024-08-16"^^xsd:date ;
    dct:source _:b15886bc6e88dcdb258fe59ded7be3abf ;
    rdfs:isDefinedBy risk: ;
    sw:term_status "accepted"@en ;
    skos:broader risk:UnauthorisedActivity ;
    skos:definition "Concept representing Unauthorised Resource Use"@en ;
    skos:inScheme risk:risk-taxonomy-classes ;
    skos:prefLabel "Unauthorised Resource Use"@en .

risk:UnauthorisedSystemAccess a rdfs:Class,
        skos:Concept,
        dpv:RiskConcept,
        risk:ConfidentialityConcept,
        risk:IntegrityConcept,
        risk:PotentialConsequence,
        risk:PotentialRisk,
        risk:PotentialRiskSource ;
    dct:contributor _:person-harshvardhan-j-pandit ;
    dct:created "2022-08-17"^^xsd:date ;
    dct:modified "2024-08-16"^^xsd:date ;
    dct:source _:b15886bc6e88dcdb258fe59ded7be3abf ;
    rdfs:isDefinedBy risk: ;
    sw:term_status "accepted"@en ;
    skos:broader risk:UnauthorisedActivity ;
    skos:definition "Concept representing Unauthorised System Access"@en ;
    skos:inScheme risk:risk-taxonomy-classes ;
    skos:prefLabel "Unauthorised System Access"@en .

risk:UnauthorisedSystemModification a rdfs:Class,
        skos:Concept,
        dpv:RiskConcept,
        risk:IntegrityConcept,
        risk:PotentialConsequence,
        risk:PotentialRisk,
        risk:PotentialRiskSource ;
    dct:contributor _:person-harshvardhan-j-pandit ;
    dct:created "2022-08-17"^^xsd:date ;
    dct:modified "2024-08-16"^^xsd:date ;
    dct:source _:bba19dc259a53f0cb59375372938fbb0a ;
    rdfs:isDefinedBy risk: ;
    sw:term_status "accepted"@en ;
    skos:broader risk:UnauthorisedActivity ;
    skos:definition "Concept representing Unauthorised System Modification"@en ;
    skos:inScheme risk:risk-taxonomy-classes ;
    skos:prefLabel "Unauthorised System Modification"@en .

risk:UnfavourableTreatment a rdfs:Class,
        skos:Concept,
        dpv:RiskConcept,
        risk:PotentialConsequence,
        risk:PotentialImpact,
        risk:PotentialRisk ;
    dct:contributor _:person-delaram-golpayegani,
        _:person-harshvardhan-j-pandit ;
    dct:created "2026-02-09"^^xsd:date ;
    rdfs:isDefinedBy risk: ;
    sw:term_status "accepted"@en ;
    skos:broader risk:Discrimination ;
    skos:definition "A treatment is unfavourable when the person(s) is treated poorly or less favorably due to specific reasons compared to other person(s)"@en ;
    skos:inScheme risk:risk-taxonomy-classes ;
    skos:prefLabel "Unfavoural Treatment"@en .

risk:UnwantedCodeDeletion a rdfs:Class,
        skos:Concept,
        dpv:RiskConcept,
        risk:AvailabilityConcept,
        risk:IntegrityConcept,
        risk:PotentialConsequence,
        risk:PotentialRisk,
        risk:PotentialRiskSource ;
    dct:contributor _:person-harshvardhan-j-pandit ;
    dct:created "2022-08-17"^^xsd:date ;
    dct:modified "2024-08-16"^^xsd:date ;
    dct:source _:bba19dc259a53f0cb59375372938fbb0a ;
    rdfs:isDefinedBy risk: ;
    sw:term_status "accepted"@en ;
    skos:broader risk:UnauthorisedActivity ;
    skos:definition "Concept representing Unwanted Code Deletion"@en ;
    skos:inScheme risk:risk-taxonomy-classes ;
    skos:prefLabel "Unwanted Code Deletion"@en .

risk:UnwantedDataDeletion a rdfs:Class,
        skos:Concept,
        dpv:RiskConcept,
        risk:AvailabilityConcept,
        risk:IntegrityConcept,
        risk:PotentialConsequence,
        risk:PotentialRisk,
        risk:PotentialRiskSource ;
    dct:contributor _:person-harshvardhan-j-pandit ;
    dct:created "2022-08-17"^^xsd:date ;
    dct:modified "2024-08-16"^^xsd:date ;
    dct:source _:b15886bc6e88dcdb258fe59ded7be3abf ;
    rdfs:isDefinedBy risk: ;
    sw:term_status "accepted"@en ;
    skos:broader risk:UnauthorisedActivity ;
    skos:definition "Concept representing Unwanted Data Deletion"@en ;
    skos:inScheme risk:risk-taxonomy-classes ;
    skos:prefLabel "Unwanted Data Deletion"@en .

risk:UnwantedDisclosureData a rdfs:Class,
        skos:Concept,
        dpv:RiskConcept,
        risk:ConfidentialityConcept,
        risk:PotentialConsequence,
        risk:PotentialRisk,
        risk:PotentialRiskSource ;
    dct:contributor _:person-harshvardhan-j-pandit ;
    dct:created "2022-08-17"^^xsd:date ;
    dct:modified "2024-08-16"^^xsd:date ;
    dct:source _:b15886bc6e88dcdb258fe59ded7be3abf ;
    rdfs:isDefinedBy risk: ;
    sw:term_status "accepted"@en ;
    skos:broader risk:UnauthorisedActivity ;
    skos:definition "Concept representing Unwanted Disclosure of Data"@en ;
    skos:inScheme risk:risk-taxonomy-classes ;
    skos:prefLabel "Unwanted Disclosure of Data"@en .

risk:UserRisks a rdfs:Class,
        skos:Concept,
        dpv:RiskConcept,
        risk:PotentialConsequence,
        risk:PotentialRisk,
        risk:PotentialRiskSource ;
    dct:created "2024-12-17"^^xsd:date ;
    rdfs:isDefinedBy risk: ;
    sw:term_status "accepted"@en ;
    skos:broader risk:OrganisationalRiskConcept ;
    skos:definition "Concepts associated with risks that arise due to User or Human use"@en ;
    skos:inScheme risk:risk-taxonomy-classes ;
    skos:prefLabel "User Risks"@en .

risk:VeryHighLikelihood a rdfs:Class,
        skos:Concept,
        dpv:Likelihood ;
    dct:contributor _:person-harshvardhan-j-pandit ;
    dct:created "2022-08-18"^^xsd:date ;
    rdf:value 0.9 ;
    rdfs:isDefinedBy risk: ;
    sw:term_status "accepted"@en ;
    skos:broader risk:5LikelihoodLevels,
        risk:7LikelihoodLevels ;
    skos:definition "Level where Likelihood is Very High"@en ;
    skos:inScheme risk:risk-levels-classes ;
    skos:prefLabel "Very High Likelihood"@en ;
    skos:scopeNote "The suggested quantitative value for this concept is 0.9 on a scale of 0 to 1"@en .

risk:VeryHighRisk a rdfs:Class,
        skos:Concept,
        dpv:RiskLevel ;
    dct:contributor _:person-harshvardhan-j-pandit ;
    dct:created "2022-08-18"^^xsd:date ;
    rdf:value 0.9 ;
    rdfs:isDefinedBy risk: ;
    sw:term_status "accepted"@en ;
    skos:broader risk:5RiskLevels,
        risk:7RiskLevels ;
    skos:definition "Level where Risk is Very High"@en ;
    skos:inScheme risk:risk-levels-classes ;
    skos:prefLabel "Very High Risk"@en ;
    skos:scopeNote "The suggested quantitative value for this concept is 0.9 on a scale of 0 to 1"@en .

risk:VeryHighSeverity a rdfs:Class,
        skos:Concept,
        dpv:Severity ;
    dct:contributor _:person-harshvardhan-j-pandit ;
    dct:created "2022-08-18"^^xsd:date ;
    rdf:value 0.9 ;
    rdfs:isDefinedBy risk: ;
    sw:term_status "accepted"@en ;
    skos:broader risk:5SeverityLevels,
        risk:7SeverityLevels ;
    skos:definition "Level where Severity is Very High"@en ;
    skos:inScheme risk:risk-levels-classes ;
    skos:prefLabel "Very High Severity"@en ;
    skos:scopeNote "The suggested quantitative value for this concept is 0.9 on a scale of 0 to 1"@en .

risk:VeryLowLikelihood a rdfs:Class,
        skos:Concept,
        dpv:Likelihood ;
    dct:contributor _:person-harshvardhan-j-pandit ;
    dct:created "2022-08-18"^^xsd:date ;
    rdf:value 0.1 ;
    rdfs:isDefinedBy risk: ;
    sw:term_status "accepted"@en ;
    skos:broader risk:5LikelihoodLevels,
        risk:7LikelihoodLevels ;
    skos:definition "Level where Likelihood is Very Low"@en ;
    skos:inScheme risk:risk-levels-classes ;
    skos:prefLabel "Very Low Likelihood"@en ;
    skos:scopeNote "The suggested quantitative value for this concept is 0.1 on a scale of 0 to 1"@en .

risk:VeryLowRisk a rdfs:Class,
        skos:Concept,
        dpv:RiskLevel ;
    dct:contributor _:person-harshvardhan-j-pandit ;
    dct:created "2022-08-18"^^xsd:date ;
    rdf:value 0.1 ;
    rdfs:isDefinedBy risk: ;
    sw:term_status "accepted"@en ;
    skos:broader risk:5RiskLevels,
        risk:7RiskLevels ;
    skos:definition "Level where Risk is Very Low"@en ;
    skos:inScheme risk:risk-levels-classes ;
    skos:prefLabel "Very Low Risk"@en ;
    skos:scopeNote "The suggested quantitative value for this concept is 0.1 on a scale of 0 to 1"@en .

risk:VeryLowSeverity a rdfs:Class,
        skos:Concept,
        dpv:Severity ;
    dct:contributor _:person-harshvardhan-j-pandit ;
    dct:created "2022-08-18"^^xsd:date ;
    rdf:value 0.1 ;
    rdfs:isDefinedBy risk: ;
    sw:term_status "accepted"@en ;
    skos:broader risk:5SeverityLevels,
        risk:7SeverityLevels ;
    skos:definition "Level where Severity is Very Low"@en ;
    skos:inScheme risk:risk-levels-classes ;
    skos:prefLabel "Very Low Severity"@en ;
    skos:scopeNote "The suggested quantitative value for this concept is 0.1 on a scale of 0 to 1"@en .

risk:ViolatingCodeOfConduct a rdfs:Class,
        skos:Concept,
        dpv:RiskConcept,
        risk:PotentialConsequence,
        risk:PotentialRisk ;
    dct:contributor _:person-harshvardhan-j-pandit ;
    dct:created "2022-08-17"^^xsd:date ;
    dct:modified "2024-08-16"^^xsd:date ;
    dct:source _:b15886bc6e88dcdb258fe59ded7be3abf ;
    rdfs:isDefinedBy risk: ;
    sw:term_status "modified"@en ;
    skos:broader risk:PolicyRisk ;
    skos:definition "Concept representing Violation of Code of Conduct"@en ;
    skos:inScheme risk:risk-taxonomy-classes ;
    skos:prefLabel "Violating Code of Conduct"@en ;
    skos:scopeNote "This concept was called \"ViolationCodeConduct\" in DPV 2.0"@en .

risk:ViolatingContractualObligation a rdfs:Class,
        skos:Concept,
        dpv:RiskConcept,
        risk:PotentialConsequence,
        risk:PotentialRisk ;
    dct:contributor _:person-harshvardhan-j-pandit ;
    dct:created "2022-08-17"^^xsd:date ;
    dct:modified "2024-08-16"^^xsd:date ;
    dct:source _:b15886bc6e88dcdb258fe59ded7be3abf ;
    rdfs:isDefinedBy risk: ;
    sw:term_status "modified"@en ;
    skos:broader risk:LegalComplianceRisk,
        risk:ViolatingObligation ;
    skos:definition "Concept representing Violation of Contractual Obligations"@en ;
    skos:inScheme risk:risk-taxonomy-classes ;
    skos:prefLabel "Violating Contractual Obligation"@en ;
    skos:scopeNote "This concept was called \"ViolationContractualObligations\" in DPV 2.0"@en .

risk:ViolatingEthicsCode a rdfs:Class,
        skos:Concept,
        dpv:RiskConcept,
        risk:PotentialConsequence,
        risk:PotentialRisk ;
    dct:contributor _:person-harshvardhan-j-pandit ;
    dct:created "2022-08-17"^^xsd:date ;
    dct:modified "2024-08-16"^^xsd:date ;
    dct:source _:b15886bc6e88dcdb258fe59ded7be3abf ;
    rdfs:isDefinedBy risk: ;
    sw:term_status "modified"@en ;
    skos:broader risk:PolicyRisk ;
    skos:definition "Concept representing Violation of Ethics Code"@en ;
    skos:inScheme risk:risk-taxonomy-classes ;
    skos:prefLabel "Violating Ethics Code"@en ;
    skos:scopeNote "This concept was called \"ViolationEthicalCode\" in DPV 2.0"@en .

risk:ViolatingLegalObligation a rdfs:Class,
        skos:Concept,
        dpv:RiskConcept,
        risk:PotentialConsequence,
        risk:PotentialRisk ;
    dct:contributor _:person-harshvardhan-j-pandit ;
    dct:created "2022-08-17"^^xsd:date ;
    dct:modified "2024-08-16"^^xsd:date ;
    dct:source _:b15886bc6e88dcdb258fe59ded7be3abf ;
    rdfs:isDefinedBy risk: ;
    sw:term_status "modified"@en ;
    skos:broader risk:LegalComplianceRisk,
        risk:ViolatingObligation ;
    skos:definition "Concept representing Violation of Legal Obligations"@en ;
    skos:inScheme risk:risk-taxonomy-classes ;
    skos:prefLabel "Violating Legal Obligation"@en ;
    skos:scopeNote "This concept was called \"ViolationRegulatoryObligations\" in DPV 2.0"@en .

risk:ViolatingObligation a rdfs:Class,
        skos:Concept,
        dpv:RiskConcept,
        risk:PotentialConsequence,
        risk:PotentialRisk ;
    dct:created "2024-10-21"^^xsd:date ;
    rdfs:isDefinedBy risk: ;
    sw:term_status "accepted"@en ;
    skos:broader risk:PolicyRisk ;
    skos:definition "Something that acts as a or violates an obligation - e.g. in a law, code of conduct, policy, contract"@en ;
    skos:inScheme risk:risk-taxonomy-classes ;
    skos:prefLabel "Violating Obligation"@en .

risk:ViolatingPolicy a rdfs:Class,
        skos:Concept,
        dpv:RiskConcept,
        risk:PotentialConsequence,
        risk:PotentialRisk ;
    dct:created "2024-12-17"^^xsd:date ;
    rdfs:isDefinedBy risk: ;
    sw:term_status "accepted"@en ;
    skos:broader risk:PolicyRisk ;
    skos:definition "Concept representing violation of policy which can be either internal or external policy"@en ;
    skos:inScheme risk:risk-taxonomy-classes ;
    skos:prefLabel "Violating Policy"@en .

risk:ViolatingProhibition a rdfs:Class,
        skos:Concept,
        dpv:RiskConcept,
        risk:PotentialConsequence,
        risk:PotentialRisk ;
    dct:created "2024-10-21"^^xsd:date ;
    rdfs:isDefinedBy risk: ;
    sw:term_status "accepted"@en ;
    skos:broader risk:PolicyRisk ;
    skos:definition "Something that acts as a or violates a prohibition - e.g. in a law, code of conduct, policy, contract"@en ;
    skos:inScheme risk:risk-taxonomy-classes ;
    skos:prefLabel "Violating Prohibition"@en .

risk:ViolatingStatutoryObligations a rdfs:Class,
        skos:Concept,
        dpv:RiskConcept,
        risk:PotentialConsequence,
        risk:PotentialRisk ;
    dct:contributor _:person-harshvardhan-j-pandit ;
    dct:created "2022-08-17"^^xsd:date ;
    dct:modified "2024-08-16"^^xsd:date ;
    dct:source _:b15886bc6e88dcdb258fe59ded7be3abf ;
    rdfs:isDefinedBy risk: ;
    sw:term_status "modified"@en ;
    skos:broader risk:LegalComplianceRisk,
        risk:ViolatingObligation ;
    skos:definition "Concept representing Violation of Statutory Obligations"@en ;
    skos:inScheme risk:risk-taxonomy-classes ;
    skos:prefLabel "Violating Statutory Obligations"@en ;
    skos:scopeNote "This concept was called \"ViolationStatutoryObligations\" in DPV 2.0"@en .

risk:ViolenceAgainstChildren a rdfs:Class,
        skos:Concept,
        dpv:RiskConcept,
        risk:PotentialConsequence,
        risk:PotentialImpact,
        risk:PotentialRisk ;
    dct:contributor _:person-harshvardhan-j-pandit ;
    dct:created "2022-08-17"^^xsd:date ;
    dct:modified "2024-08-16"^^xsd:date ;
    dct:source _:b7191aa21b975cb14bbce32aa3ba9c7eb ;
    rdfs:isDefinedBy risk: ;
    sw:term_status "accepted"@en ;
    skos:broader risk:Harm ;
    skos:definition "Concept representing Child Violence"@en ;
    skos:inScheme risk:risk-taxonomy-classes ;
    skos:prefLabel "Violence against children"@en ;
    skos:scopeNote "This concept was called \"ChildViolence\" in DPV 2.0"@en .

risk:Vulnerability a rdfs:Class,
        skos:Concept ;
    dct:created "2024-02-14"^^xsd:date ;
    rdfs:isDefinedBy risk: ;
    rdfs:subClassOf risk:RiskIdentification ;
    sw:term_status "accepted"@en ;
    skos:broader risk:RiskIdentification ;
    skos:definition "Intrinsic property of a system or asset that is utilised by the Threat Source in a Threat event to cause Risk"@en ;
    skos:inScheme risk:risk-management-classes ;
    skos:prefLabel "Vulnerability"@en .

risk:VulnerabilityExploitation a rdfs:Class,
        skos:Concept,
        dpv:RiskConcept,
        risk:PotentialConsequence,
        risk:PotentialRisk,
        risk:PotentialRiskSource ;
    dct:contributor _:person-delaram-golpayegani,
        _:person-harshvardhan-j-pandit ;
    dct:created "2026-02-09"^^xsd:date ;
    rdfs:isDefinedBy risk: ;
    sw:term_status "accepted"@en ;
    skos:broader risk:MaliciousActivity ;
    skos:definition "Concept representing Vulnerability Exploitation"@en ;
    skos:inScheme risk:risk-taxonomy-classes ;
    skos:prefLabel "Vulnerability Exploitation"@en .

risk:Wellbeing a rdfs:Class,
        skos:Concept,
        dpv:RiskConcept,
        risk:PotentialConsequence,
        risk:PotentialImpact,
        risk:PotentialRisk ;
    dct:contributor _:person-delaram-golpayegani ;
    dct:created "2024-12-01"^^xsd:date ;
    rdfs:isDefinedBy risk: ;
    sw:term_status "accepted"@en ;
    skos:broader risk:HealthSafety ;
    skos:definition "Concept representing wellbeing of individual(s)"@en ;
    skos:inScheme risk:risk-taxonomy-classes ;
    skos:prefLabel "Wellbeing"@en .

risk:WorkplaceDiscrimination a rdfs:Class,
        skos:Concept,
        dpv:RiskConcept,
        risk:PotentialConsequence,
        risk:PotentialImpact,
        risk:PotentialRisk ;
    dct:contributor _:person-harshvardhan-j-pandit ;
    dct:created "2024-12-01"^^xsd:date ;
    rdfs:isDefinedBy risk: ;
    sw:term_status "accepted"@en ;
    skos:broader risk:Discrimination ;
    skos:definition "Discrimination occurring at workplace or in the context of work environments"@en ;
    skos:inScheme risk:risk-taxonomy-classes ;
    skos:prefLabel "Workplace Discrimination"@en .

<https://w3id.org/dpv/risk> a owl:Ontology,
        profile:Profile ;
    dct:bibliographicCitation "Harshvardhan J. Pandit, Beatriz Esteves, Georg P. Krog, Paul Ryan, Delaram Golpayegani, Julian Flake (2025) Data Privacy Vocabulary (DPV)  Version 2.0. In: Demartini, G., et al. The Semantic Web  ISWC 2024. ISWC 2024. Lecture Notes in Computer Science, vol 15233. Springer, Cham. https://doi.org/10.1007/978-3-031-77847-6_10" ;
    dct:conformsTo "http://www.w3.org/2000/01/rdf-schema",
        "http://www.w3.org/2004/02/skos/core" ;
    dct:contributor _:person-arthit-suriyawongkul,
        _:person-axel-polleres,
        _:person-beatriz-esteves,
        _:person-daniel-doherty,
        _:person-delaram-golpayegani,
        _:person-fajar-ekaputra,
        _:person-georg-p-krog,
        _:person-harshvardhan-j-pandit,
        _:person-julian-flake,
        _:person-julio-hernandez,
        _:person-rob-brennan ;
    dct:created "2022-08-14"@en ;
    dct:creator _:person-beatriz-esteves,
        _:person-delaram-golpayegani,
        _:person-georg-p-krog,
        _:person-harshvardhan-j-pandit,
        _:person-julian-flake,
        [ a dct:Agent,
                foaf:Person ;
            scoro:hasORCID "0000-0003-0770-2737" ;
            org:memberOf [ a foaf:Organization ;
                    foaf:name "Uniphar PLC" ] ;
            foaf:name "Paul Ryan" ],
        _:person-rob-brennan ;
    dct:description "Extension to the Data Privacy Vocabulary (DPV) providing concepts for representing information about risk assessment and risk management"@en ;
    dct:identifier "https://w3id.org/dpv/risk" ;
    dct:issued "2022-08-14"@en ;
    dct:license <https://www.w3.org/copyright/document-license-2023/> ;
    dct:modified "2026-02-25"@en ;
    dct:publisher <https://www.w3.org/> ;
    dct:source <https://www.w3.org/groups/cg/dpvcg/> ;
    dct:title "Risk Concepts"@en ;
    bibo:doi "10.5281/zenodo.12505841" ;
    bibo:status "http://purl.org/ontology/bibo/status/published" ;
    vann:preferredNamespacePrefix "risk" ;
    vann:preferredNamespaceUri "https://w3id.org/dpv/risk#" ;
    rdfs:Label "RISK"@en ;
    owl:versionIRI <https://w3id.org/dpv/2.3/risk> ;
    owl:versionInfo "2.3" ;
    profile:hasResource <https://w3id.org/dpv/examples>,
        <https://w3id.org/dpv/guides>,
        <https://w3id.org/dpv/primer>,
        risk:serialisation-html,
        risk:serialisation-ttl ;
    profile:isProfileOf rdfs:,
        skos:,
        <https://w3id.org/dpv> ;
    foaf:logo <https://w3id.org/dpv/media/logo.png> ;
    schema:version "2.3" .

risk:causedByThreat a rdf:Property,
        skos:Concept ;
    dcam:rangeIncludes risk:Threat ;
    dct:created "2024-02-14"^^xsd:date ;
    rdfs:isDefinedBy risk: ;
    sw:term_status "accepted"@en ;
    skos:definition "Indicates the cause of associated context (subject) was the indicated threat (object)"@en ;
    skos:inScheme risk:risk-management-properties ;
    skos:prefLabel "caused by threat"@en ;
    schema:rangeIncludes risk:Threat .

risk:causedByVulnerability a rdf:Property,
        skos:Concept ;
    dcam:rangeIncludes risk:Vulnerability ;
    dct:created "2024-02-14"^^xsd:date ;
    rdfs:isDefinedBy risk: ;
    sw:term_status "accepted"@en ;
    skos:definition "Indicates the associated context (subject) is caused by the indicated vulnerability (object)"@en ;
    skos:inScheme risk:risk-management-properties ;
    skos:prefLabel "caused by vulnerability"@en ;
    schema:rangeIncludes risk:Vulnerability .

risk:contains a rdf:Property,
        skos:Concept ;
    dcam:domainIncludes risk:ContainmentControl ;
    dcam:rangeIncludes dpv:RiskConcept ;
    dct:contributor _:person-harshvardhan-j-pandit ;
    dct:created "2025-01-06"^^xsd:date ;
    rdfs:isDefinedBy risk: ;
    rdfs:subPropertyOf risk:controls ;
    sw:term_status "accepted"@en ;
    skos:broader risk:controls ;
    skos:definition "Indicates the specified event or action is contained by this control"@en ;
    skos:inScheme risk:risk-controls-properties ;
    skos:prefLabel "contains"@en ;
    schema:domainIncludes risk:ContainmentControl ;
    schema:rangeIncludes dpv:RiskConcept .

risk:detects a rdf:Property,
        skos:Concept ;
    dcam:domainIncludes risk:DetectionControl ;
    dcam:rangeIncludes dpv:RiskConcept ;
    dct:contributor _:person-delaram-golpayegani,
        _:person-harshvardhan-j-pandit ;
    dct:created "2024-12-01"^^xsd:date ;
    dct:modified "2025-01-06"^^xsd:date ;
    rdfs:isDefinedBy risk: ;
    rdfs:subPropertyOf risk:monitors ;
    sw:term_status "modified"@en ;
    skos:broader risk:monitors ;
    skos:definition "Indicates the specified event or action is detected by this control"@en ;
    skos:inScheme risk:risk-controls-properties ;
    skos:prefLabel "detects"@en ;
    schema:domainIncludes risk:DetectionControl ;
    schema:rangeIncludes dpv:RiskConcept .

risk:eliminates a rdf:Property,
        skos:Concept ;
    dcam:domainIncludes risk:EliminationControl ;
    dcam:rangeIncludes dpv:RiskConcept ;
    dct:contributor _:person-delaram-golpayegani,
        _:person-harshvardhan-j-pandit ;
    dct:created "2024-12-01"^^xsd:date ;
    dct:modified "2025-01-06"^^xsd:date ;
    rdfs:isDefinedBy risk: ;
    rdfs:subPropertyOf risk:avoids ;
    sw:term_status "modified"@en ;
    skos:broader risk:avoids ;
    skos:definition "Indicates the specified event or action is eliminated by this control"@en ;
    skos:inScheme risk:risk-controls-properties ;
    skos:prefLabel "eliminates"@en ;
    schema:domainIncludes risk:EliminationControl ;
    schema:rangeIncludes dpv:RiskConcept .

risk:exploitsVulnerability a rdf:Property,
        skos:Concept ;
    dcam:domainIncludes risk:Threat ;
    dcam:rangeIncludes risk:Vulnerability ;
    dct:created "2024-02-14"^^xsd:date ;
    rdfs:isDefinedBy risk: ;
    sw:term_status "accepted"@en ;
    skos:definition "Indicates the threat (subject) exploits the indicated vulnerability (object)"@en ;
    skos:inScheme risk:risk-management-properties ;
    skos:prefLabel "exploits vulnerability"@en ;
    schema:domainIncludes risk:Threat ;
    schema:rangeIncludes risk:Vulnerability .

risk:hasControl a rdf:Property,
        skos:Concept ;
    dcam:rangeIncludes risk:RiskControl ;
    dct:contributor _:person-harshvardhan-j-pandit ;
    dct:created "2024-02-14"^^xsd:date ;
    dct:modified "2025-01-06"^^xsd:date ;
    vann:example dex:E0071 ;
    rdfs:isDefinedBy risk: ;
    sw:term_status "modified"@en ;
    skos:definition "Indicates the use of specified control"@en ;
    skos:inScheme risk:risk-controls-properties ;
    skos:prefLabel "has control"@en ;
    schema:rangeIncludes risk:RiskControl .

risk:hasIncident a rdf:Property,
        skos:Concept ;
    dcam:rangeIncludes risk:Incident ;
    dct:created "2024-02-14"^^xsd:date ;
    rdfs:isDefinedBy risk: ;
    sw:term_status "accepted"@en ;
    skos:definition "Indicates an incident is associated with the specified context"@en ;
    skos:inScheme risk:incident-properties ;
    skos:prefLabel "has incident"@en ;
    schema:rangeIncludes risk:Incident .

risk:hasRiskAcceptance a rdf:Property,
        skos:Concept ;
    dcam:rangeIncludes risk:RiskAcceptance ;
    dct:created "2024-12-01"^^xsd:date ;
    rdfs:isDefinedBy risk: ;
    sw:term_status "accepted"@en ;
    skos:definition "Associates the risk acceptance plan or process or criteria"@en ;
    skos:inScheme risk:risk-management-properties ;
    skos:prefLabel "has risk acceptance"@en ;
    schema:rangeIncludes risk:RiskAcceptance .

risk:hasRiskAnalysis a rdf:Property,
        skos:Concept ;
    dcam:rangeIncludes risk:RiskAnalysis ;
    dct:created "2024-12-01"^^xsd:date ;
    rdfs:isDefinedBy risk: ;
    sw:term_status "accepted"@en ;
    skos:definition "Associates the risk analysis"@en ;
    skos:inScheme risk:risk-management-properties ;
    skos:prefLabel "has risk analysis"@en ;
    schema:rangeIncludes risk:RiskAnalysis .

risk:hasRiskAssessment a rdf:Property,
        skos:Concept ;
    dcam:rangeIncludes risk:RiskAssessment ;
    dct:created "2024-12-01"^^xsd:date ;
    rdfs:isDefinedBy risk: ;
    sw:term_status "accepted"@en ;
    skos:definition "Associates the risk assessment"@en ;
    skos:inScheme risk:risk-management-properties ;
    skos:prefLabel "has risk assessment"@en ;
    schema:rangeIncludes risk:RiskAssessment .

risk:hasRiskCriteria a rdf:Property,
        skos:Concept ;
    dcam:rangeIncludes risk:RiskCriteria ;
    dct:created "2024-12-01"^^xsd:date ;
    rdfs:isDefinedBy risk: ;
    sw:term_status "accepted"@en ;
    skos:definition "Associates the risk criteria"@en ;
    skos:inScheme risk:risk-management-properties ;
    skos:prefLabel "has risk criteria"@en ;
    schema:rangeIncludes risk:RiskCriteria .

risk:hasRiskEvaluation a rdf:Property,
        skos:Concept ;
    dcam:rangeIncludes risk:RiskEvaluation ;
    dct:created "2024-12-01"^^xsd:date ;
    rdfs:isDefinedBy risk: ;
    sw:term_status "accepted"@en ;
    skos:definition "Associates the risk evaluation plan or process or criteria"@en ;
    skos:inScheme risk:risk-management-properties ;
    skos:prefLabel "has risk evaluation"@en ;
    schema:rangeIncludes risk:RiskEvaluation .

risk:hasRiskIdentification a rdf:Property,
        skos:Concept ;
    dcam:rangeIncludes risk:RiskIdentification ;
    dct:created "2024-12-01"^^xsd:date ;
    rdfs:isDefinedBy risk: ;
    sw:term_status "accepted"@en ;
    skos:definition "Associates the risk identification plan or process or criteria"@en ;
    skos:inScheme risk:risk-management-properties ;
    skos:prefLabel "has risk identification"@en ;
    schema:rangeIncludes risk:RiskIdentification .

risk:hasRiskManagement a rdf:Property,
        skos:Concept ;
    dcam:rangeIncludes risk:RiskManagement ;
    dct:created "2024-12-01"^^xsd:date ;
    rdfs:isDefinedBy risk: ;
    sw:term_status "accepted"@en ;
    skos:definition "Associates the risk management plan or process"@en ;
    skos:inScheme risk:risk-management-properties ;
    skos:prefLabel "has risk management"@en ;
    schema:rangeIncludes risk:RiskManagement .

risk:hasRiskOwner a rdf:Property,
        skos:Concept ;
    dcam:rangeIncludes risk:RiskOwner ;
    dct:created "2024-12-01"^^xsd:date ;
    rdfs:isDefinedBy risk: ;
    sw:term_status "accepted"@en ;
    skos:definition "Indicates the risk owner"@en ;
    skos:inScheme risk:risk-management-properties ;
    skos:prefLabel "has risk owner"@en ;
    schema:rangeIncludes risk:RiskOwner .

risk:hasRiskPerception a rdf:Property,
        skos:Concept ;
    dcam:rangeIncludes risk:RiskPerception ;
    dct:created "2024-12-01"^^xsd:date ;
    rdfs:isDefinedBy risk: ;
    sw:term_status "accepted"@en ;
    skos:definition "Associates the risk perception plan or process or criteria"@en ;
    skos:inScheme risk:risk-management-properties ;
    skos:prefLabel "has risk perception"@en ;
    schema:rangeIncludes risk:RiskPerception .

risk:hasRiskSource a rdf:Property,
        skos:Concept ;
    dcam:domainIncludes dpv:Risk ;
    dcam:rangeIncludes risk:RiskSource ;
    dct:created "2024-02-14"^^xsd:date ;
    rdfs:isDefinedBy risk: ;
    sw:term_status "accepted"@en ;
    skos:definition "Indicates the risk (subject) has the indicated risk source (object)"@en ;
    skos:inScheme risk:risk-management-properties ;
    skos:prefLabel "has risk source"@en ;
    schema:domainIncludes dpv:Risk ;
    schema:rangeIncludes risk:RiskSource .

risk:hasRiskTreatment a rdf:Property,
        skos:Concept ;
    dcam:rangeIncludes risk:RiskTreatment ;
    dct:created "2024-12-01"^^xsd:date ;
    rdfs:isDefinedBy risk: ;
    sw:term_status "accepted"@en ;
    skos:definition "Associates the risk treatment plan or process or criteria"@en ;
    skos:inScheme risk:risk-management-properties ;
    skos:prefLabel "has risk treatment"@en ;
    schema:rangeIncludes risk:RiskTreatment .

risk:hasThreatSource a rdf:Property,
        skos:Concept ;
    dcam:domainIncludes risk:Threat ;
    dcam:rangeIncludes risk:ThreatSource ;
    dct:created "2024-02-14"^^xsd:date ;
    rdfs:isDefinedBy risk: ;
    sw:term_status "accepted"@en ;
    skos:definition "Indicates the threat (subject) has the indicated source (object)"@en ;
    skos:inScheme risk:risk-management-properties ;
    skos:prefLabel "has threat source"@en ;
    schema:domainIncludes risk:Threat ;
    schema:rangeIncludes risk:ThreatSource .

risk:hasVulnerability a rdf:Property,
        skos:Concept ;
    dcam:rangeIncludes risk:Vulnerability ;
    dct:created "2024-02-14"^^xsd:date ;
    rdfs:isDefinedBy risk: ;
    sw:term_status "accepted"@en ;
    skos:definition "Indicates the associated context (subject) has indicated vulnerability (object)"@en ;
    skos:inScheme risk:risk-management-properties ;
    skos:prefLabel "has vulnerability"@en ;
    schema:rangeIncludes risk:Vulnerability .

risk:identifies a rdf:Property,
        skos:Concept ;
    dcam:domainIncludes risk:IdentificationControl ;
    dcam:rangeIncludes dpv:RiskConcept ;
    dct:contributor _:person-delaram-golpayegani,
        _:person-harshvardhan-j-pandit ;
    dct:created "2024-12-01"^^xsd:date ;
    dct:modified "2025-01-06"^^xsd:date ;
    rdfs:isDefinedBy risk: ;
    rdfs:subPropertyOf risk:monitors ;
    sw:term_status "modified"@en ;
    skos:broader risk:monitors ;
    skos:definition "Indicates the specified event or action is identified by this control"@en ;
    skos:inScheme risk:risk-controls-properties ;
    skos:prefLabel "identifies"@en ;
    schema:domainIncludes risk:IdentificationControl ;
    schema:rangeIncludes dpv:RiskConcept .

risk:interrupts a rdf:Property,
        skos:Concept ;
    dcam:domainIncludes risk:InterruptionControl ;
    dcam:rangeIncludes dpv:RiskConcept ;
    dct:contributor _:person-harshvardhan-j-pandit ;
    dct:created "2025-01-06"^^xsd:date ;
    rdfs:isDefinedBy risk: ;
    rdfs:subPropertyOf risk:reduces ;
    sw:term_status "accepted"@en ;
    skos:broader risk:reduces ;
    skos:definition "Indicates the specified event or action is interrupted by this control"@en ;
    skos:inScheme risk:risk-controls-properties ;
    skos:prefLabel "interrupts"@en ;
    schema:domainIncludes risk:InterruptionControl ;
    schema:rangeIncludes dpv:RiskConcept .

risk:intervenes a rdf:Property,
        skos:Concept ;
    dcam:domainIncludes risk:InterventionControl ;
    dcam:rangeIncludes dpv:RiskConcept ;
    dct:contributor _:person-harshvardhan-j-pandit ;
    dct:created "2025-01-06"^^xsd:date ;
    rdfs:isDefinedBy risk: ;
    rdfs:subPropertyOf risk:reduces ;
    sw:term_status "accepted"@en ;
    skos:broader risk:reduces ;
    skos:definition "Indicates the specified event or action is intervened by this control"@en ;
    skos:inScheme risk:risk-controls-properties ;
    skos:prefLabel "intervenes"@en ;
    schema:domainIncludes risk:InterventionControl ;
    schema:rangeIncludes dpv:RiskConcept .

risk:investigates a rdf:Property,
        skos:Concept ;
    dcam:domainIncludes risk:InvestigationControl ;
    dcam:rangeIncludes dpv:RiskConcept ;
    dct:contributor _:person-harshvardhan-j-pandit ;
    dct:created "2025-01-06"^^xsd:date ;
    rdfs:isDefinedBy risk: ;
    rdfs:subPropertyOf risk:controls ;
    sw:term_status "accepted"@en ;
    skos:broader risk:controls ;
    skos:definition "Indicates the specified event or action is investigated by this control"@en ;
    skos:inScheme risk:risk-controls-properties ;
    skos:prefLabel "investigates"@en ;
    schema:domainIncludes risk:InvestigationControl ;
    schema:rangeIncludes dpv:RiskConcept .

risk:isExploitedBy a rdf:Property,
        skos:Concept ;
    dcam:domainIncludes risk:Vulnerability ;
    dcam:rangeIncludes risk:Threat ;
    dct:created "2024-02-14"^^xsd:date ;
    rdfs:isDefinedBy risk: ;
    sw:term_status "accepted"@en ;
    skos:definition "Indicates the vulnerability (subject) is exploited by the indicated threat (object)"@en ;
    skos:inScheme risk:risk-management-properties ;
    skos:prefLabel "is exploited by"@en ;
    schema:domainIncludes risk:Vulnerability ;
    schema:rangeIncludes risk:Threat .

risk:isVulnerabilityOf a rdf:Property,
        skos:Concept ;
    dcam:domainIncludes risk:Vulnerability ;
    dct:created "2024-02-14"^^xsd:date ;
    rdfs:isDefinedBy risk: ;
    sw:term_status "accepted"@en ;
    skos:definition "Indicates the vulnerability (subject) is associated with indicated context (object)"@en ;
    skos:inScheme risk:risk-management-properties ;
    skos:prefLabel "is vulnerability of"@en ;
    schema:domainIncludes risk:Vulnerability .

risk:logs a rdf:Property,
        skos:Concept ;
    dcam:domainIncludes risk:LoggingControl ;
    dcam:rangeIncludes dpv:RiskConcept ;
    dct:contributor _:person-harshvardhan-j-pandit ;
    dct:created "2025-01-06"^^xsd:date ;
    rdfs:isDefinedBy risk: ;
    rdfs:subPropertyOf risk:monitors ;
    sw:term_status "accepted"@en ;
    skos:broader risk:monitors ;
    skos:definition "Indicates the specified event or action is logged by this control"@en ;
    skos:inScheme risk:risk-controls-properties ;
    skos:prefLabel "logs"@en ;
    schema:domainIncludes risk:LoggingControl ;
    schema:rangeIncludes dpv:RiskConcept .

risk:mitigates a rdf:Property,
        skos:Concept ;
    dcam:domainIncludes risk:MitigationControl ;
    dcam:rangeIncludes dpv:RiskConcept ;
    dct:contributor _:person-delaram-golpayegani,
        _:person-harshvardhan-j-pandit ;
    dct:created "2024-12-01"^^xsd:date ;
    dct:modified "2025-01-06"^^xsd:date ;
    rdfs:isDefinedBy risk: ;
    rdfs:subPropertyOf risk:avoids ;
    sw:term_status "modified"@en ;
    skos:broader risk:avoids ;
    skos:definition "Indicates the specified event or action is mitigated by this control"@en ;
    skos:inScheme risk:risk-controls-properties ;
    skos:prefLabel "mitigates"@en ;
    schema:domainIncludes risk:MitigationControl ;
    schema:rangeIncludes dpv:RiskConcept .

risk:modifies a rdf:Property,
        skos:Concept ;
    dcam:domainIncludes risk:ModificationControl ;
    dcam:rangeIncludes dpv:RiskConcept ;
    dct:contributor _:person-delaram-golpayegani,
        _:person-harshvardhan-j-pandit ;
    dct:created "2024-12-01"^^xsd:date ;
    dct:modified "2025-01-06"^^xsd:date ;
    rdfs:isDefinedBy risk: ;
    rdfs:subPropertyOf risk:avoids ;
    sw:term_status "modified"@en ;
    skos:broader risk:avoids ;
    skos:definition "Indicates the specified event or action is modified by this control"@en ;
    skos:inScheme risk:risk-controls-properties ;
    skos:prefLabel "modifies"@en ;
    schema:domainIncludes risk:ModificationControl ;
    schema:rangeIncludes dpv:RiskConcept .

risk:overrides a rdf:Property,
        skos:Concept ;
    dcam:domainIncludes risk:OverrideControl ;
    dcam:rangeIncludes dpv:RiskConcept ;
    dct:contributor _:person-harshvardhan-j-pandit ;
    dct:created "2025-01-06"^^xsd:date ;
    rdfs:isDefinedBy risk: ;
    rdfs:subPropertyOf risk:controls ;
    sw:term_status "accepted"@en ;
    skos:broader risk:controls ;
    skos:definition "Indicates the specified event or action is overridden by this control"@en ;
    skos:inScheme risk:risk-controls-properties ;
    skos:prefLabel "overrides"@en ;
    schema:domainIncludes risk:OverrideControl ;
    schema:rangeIncludes dpv:RiskConcept .

risk:recovers a rdf:Property,
        skos:Concept ;
    dcam:domainIncludes risk:RecoveryControl ;
    dcam:rangeIncludes dpv:RiskConcept ;
    dct:contributor _:person-harshvardhan-j-pandit ;
    dct:created "2025-01-06"^^xsd:date ;
    rdfs:isDefinedBy risk: ;
    rdfs:subPropertyOf risk:resolves ;
    sw:term_status "accepted"@en ;
    skos:broader risk:resolves ;
    skos:definition "Indicates the specified event or action is recovered from by this control"@en ;
    skos:inScheme risk:risk-controls-properties ;
    skos:prefLabel "recovers"@en ;
    schema:domainIncludes risk:RecoveryControl ;
    schema:rangeIncludes dpv:RiskConcept .

risk:refersToRisk a rdf:Property,
        skos:Concept ;
    dcam:domainIncludes dpv:Incident ;
    dcam:rangeIncludes dpv:Risk ;
    dct:created "2024-02-14"^^xsd:date ;
    vann:example dex:E0069 ;
    rdfs:isDefinedBy risk: ;
    sw:term_status "accepted"@en ;
    skos:definition "Indicates the incident (subject) is a materialisation of the indicated risk (object)"@en ;
    skos:inScheme risk:risk-management-properties ;
    skos:prefLabel "refers to risk"@en ;
    schema:domainIncludes dpv:Incident ;
    schema:rangeIncludes dpv:Risk .

risk:remedies a rdf:Property,
        skos:Concept ;
    dcam:domainIncludes risk:RemediationControl ;
    dcam:rangeIncludes dpv:RiskConcept ;
    dct:contributor _:person-harshvardhan-j-pandit ;
    dct:created "2025-01-06"^^xsd:date ;
    rdfs:isDefinedBy risk: ;
    rdfs:subPropertyOf risk:resolves ;
    sw:term_status "accepted"@en ;
    skos:broader risk:resolves ;
    skos:definition "Indicates the specified event or action is remedied by this control"@en ;
    skos:inScheme risk:risk-controls-properties ;
    skos:prefLabel "remedies"@en ;
    schema:domainIncludes risk:RemediationControl ;
    schema:rangeIncludes dpv:RiskConcept .

risk:reverses a rdf:Property,
        skos:Concept ;
    dcam:domainIncludes risk:ReversalControl ;
    dcam:rangeIncludes dpv:RiskConcept ;
    dct:contributor _:person-harshvardhan-j-pandit ;
    dct:created "2025-01-06"^^xsd:date ;
    rdfs:isDefinedBy risk: ;
    rdfs:subPropertyOf risk:resolves ;
    sw:term_status "accepted"@en ;
    skos:broader risk:resolves ;
    skos:definition "Indicates the specified event or action is reversed by this control"@en ;
    skos:inScheme risk:risk-controls-properties ;
    skos:prefLabel "reverses"@en ;
    schema:domainIncludes risk:ReversalControl ;
    schema:rangeIncludes dpv:RiskConcept .

risk:shares a rdf:Property,
        skos:Concept ;
    dcam:domainIncludes risk:ShareControl ;
    dcam:rangeIncludes dpv:RiskConcept ;
    dct:contributor _:person-harshvardhan-j-pandit ;
    dct:created "2025-01-06"^^xsd:date ;
    rdfs:isDefinedBy risk: ;
    rdfs:subPropertyOf risk:controls ;
    sw:term_status "accepted"@en ;
    skos:broader risk:controls ;
    skos:definition "Indicates the specified event or action is shared with another context or entity by this control"@en ;
    skos:inScheme risk:risk-controls-properties ;
    skos:prefLabel "shares"@en ;
    schema:domainIncludes risk:ShareControl ;
    schema:rangeIncludes dpv:RiskConcept .

risk:substitutes a rdf:Property,
        skos:Concept ;
    dcam:domainIncludes risk:SubstitutionControl ;
    dcam:rangeIncludes dpv:RiskConcept ;
    dct:contributor _:person-harshvardhan-j-pandit ;
    dct:created "2025-01-06"^^xsd:date ;
    rdfs:isDefinedBy risk: ;
    rdfs:subPropertyOf risk:avoids ;
    sw:term_status "accepted"@en ;
    skos:broader risk:avoids ;
    skos:definition "Indicates the specified event or action is substituted by this control"@en ;
    skos:inScheme risk:risk-controls-properties ;
    skos:prefLabel "substitutes"@en ;
    schema:domainIncludes risk:SubstitutionControl ;
    schema:rangeIncludes dpv:RiskConcept .

risk:transfers a rdf:Property,
        skos:Concept ;
    dcam:domainIncludes risk:TransferControl ;
    dcam:rangeIncludes dpv:RiskConcept ;
    dct:contributor _:person-harshvardhan-j-pandit ;
    dct:created "2025-01-06"^^xsd:date ;
    rdfs:isDefinedBy risk: ;
    rdfs:subPropertyOf risk:controls ;
    sw:term_status "accepted"@en ;
    skos:broader risk:controls ;
    skos:definition "Indicates the specified event or action is transferred to another context or entity by this control"@en ;
    skos:inScheme risk:risk-controls-properties ;
    skos:prefLabel "transfers"@en ;
    schema:domainIncludes risk:TransferControl ;
    schema:rangeIncludes dpv:RiskConcept .

risk:incident-properties a skos:ConceptScheme .

risk:serialisation-html a profile:ResourceDescriptor ;
    dct:conformsTo <https://www.w3.org/TR/html/> ;
    dct:format <https://www.iana.org/assignments/media-types/text/html> ;
    dct:title "Risk Concepts - HTML serialisation" ;
    profile:hasArtifact <https://w3id.org/dpv/risk/risk.html> ;
    profile:hasRole role:specification .

risk:serialisation-ttl a profile:ResourceDescriptor ;
    dct:conformsTo <https://www.w3.org/TR/turtle/> ;
    dct:format <https://www.iana.org/assignments/media-types/text/turtle> ;
    dct:title "Risk Concepts - Turtle serialisation" ;
    profile:hasArtifact <https://w3id.org/dpv/risk/risk.ttl> ;
    profile:hasRole role:vocabulary .

<https://w3id.org/dpv/examples> a profile:ResourceDescriptor ;
    dct:conformsTo <https://www.w3.org/TR/html/> ;
    dct:format <https://www.iana.org/assignments/media-types/text/html> ;
    dct:title "Examples" ;
    profile:hasArtifact <https://w3id.org/dpv/examples> ;
    profile:hasRole role:guidance .

<https://w3id.org/dpv/guides> a profile:ResourceDescriptor ;
    dct:conformsTo <https://www.w3.org/TR/html/> ;
    dct:format <https://www.iana.org/assignments/media-types/text/html> ;
    dct:title "Guides for Data Privacy Vocabulary" ;
    profile:hasArtifact <https://w3id.org/dpv/guides> ;
    profile:hasRole role:guidance .

<https://w3id.org/dpv/primer> a profile:ResourceDescriptor ;
    dct:conformsTo <https://www.w3.org/TR/html/> ;
    dct:format <https://www.iana.org/assignments/media-types/text/html> ;
    dct:title "Primer for Data Privacy Vocabulary" ;
    profile:hasArtifact <https://w3id.org/dpv/primer> ;
    profile:hasRole role:guidance .

risk:monitors a rdf:Property,
        skos:Concept ;
    dcam:domainIncludes risk:MonitorControl ;
    dcam:rangeIncludes dpv:RiskConcept ;
    dct:contributor _:person-harshvardhan-j-pandit ;
    dct:created "2025-01-06"^^xsd:date ;
    rdfs:isDefinedBy risk: ;
    rdfs:subPropertyOf risk:controls ;
    sw:term_status "accepted"@en ;
    skos:broader risk:controls ;
    skos:definition "Indicates the specified event or action is monitored by this control"@en ;
    skos:inScheme risk:risk-controls-properties ;
    skos:prefLabel "monitors"@en ;
    schema:domainIncludes risk:MonitorControl ;
    schema:rangeIncludes dpv:RiskConcept .

risk:reduces a rdf:Property,
        skos:Concept ;
    dcam:domainIncludes risk:ReductionControl ;
    dcam:rangeIncludes dpv:RiskConcept ;
    dct:contributor _:person-harshvardhan-j-pandit ;
    dct:created "2025-01-06"^^xsd:date ;
    rdfs:isDefinedBy risk: ;
    rdfs:subPropertyOf risk:controls ;
    sw:term_status "accepted"@en ;
    skos:broader risk:controls ;
    skos:definition "Indicates the specified event or action is reduced by this control"@en ;
    skos:inScheme risk:risk-controls-properties ;
    skos:prefLabel "reduces"@en ;
    schema:domainIncludes risk:ReductionControl ;
    schema:rangeIncludes dpv:RiskConcept .

risk:resolves a rdf:Property,
        skos:Concept ;
    dcam:domainIncludes risk:ResolutionControl ;
    dcam:rangeIncludes dpv:RiskConcept ;
    dct:contributor _:person-harshvardhan-j-pandit ;
    dct:created "2025-01-06"^^xsd:date ;
    rdfs:isDefinedBy risk: ;
    rdfs:subPropertyOf risk:controls ;
    sw:term_status "accepted"@en ;
    skos:broader risk:controls ;
    skos:definition "Indicates the specified event or action is resolved by this control"@en ;
    skos:inScheme risk:risk-controls-properties ;
    skos:prefLabel "resolves"@en ;
    schema:domainIncludes risk:ResolutionControl ;
    schema:rangeIncludes dpv:RiskConcept .

risk:avoids a rdf:Property,
        skos:Concept ;
    dcam:domainIncludes risk:AvoidanceControl ;
    dcam:rangeIncludes dpv:RiskConcept ;
    dct:contributor _:person-harshvardhan-j-pandit ;
    dct:created "2025-01-06"^^xsd:date ;
    rdfs:isDefinedBy risk: ;
    rdfs:subPropertyOf risk:reduces ;
    sw:term_status "accepted"@en ;
    skos:broader risk:reduces ;
    skos:definition "Indicates the event or action is avoided by the specified control"@en ;
    skos:inScheme risk:risk-controls-properties ;
    skos:prefLabel "avoids"@en ;
    schema:domainIncludes risk:AvoidanceControl ;
    schema:rangeIncludes dpv:RiskConcept .

risk:incident-status-classes a skos:ConceptScheme .

risk:risk-management-classes a skos:ConceptScheme .

risk:controls a rdf:Property,
        skos:Concept ;
    dcam:domainIncludes risk:RiskControl ;
    dcam:rangeIncludes dpv:RiskConcept ;
    dct:contributor _:person-harshvardhan-j-pandit ;
    dct:created "2025-01-06"^^xsd:date ;
    vann:example dex:E0086 ;
    rdfs:isDefinedBy risk: ;
    sw:term_status "accepted"@en ;
    skos:definition "Indicates this control manages specified risk concept event or action, such as for risk sources, risks, consequences, and impacts"@en ;
    skos:inScheme risk:risk-controls-properties ;
    skos:prefLabel "control"@en ;
    schema:domainIncludes risk:RiskControl ;
    schema:rangeIncludes dpv:RiskConcept .

risk:risk-management-properties a skos:ConceptScheme .

risk:incident-classes a skos:ConceptScheme .

risk:risk-controls-properties a skos:ConceptScheme .

risk:risk-levels-classes a skos:ConceptScheme .

risk:risk-controls-classes a skos:ConceptScheme .

risk:risk-matrix-classes a skos:ConceptScheme .

risk:risk-taxonomy-classes a skos:ConceptScheme .

_:org-ai-accountability-lab-aial-trinity-college-dublin a foaf:Organization ;
    foaf:name "AI Accountability Lab (AIAL), Trinity College Dublin" .

_:org-dublin-city-university a foaf:Organization ;
    foaf:name "Dublin City University" .

_:org-idlab-imec-ghent-university a foaf:Organization ;
    foaf:name "IDLab, IMEC, Ghent University" .

_:org-signatu-as a foaf:Organization ;
    foaf:name "Signatu AS" .

_:org-trinity-college-dublin a foaf:Organization ;
    foaf:name "Trinity College Dublin" .

_:org-university-college-dublin a foaf:Organization ;
    foaf:name "University College Dublin" .

_:org-university-of-koblenz a foaf:Organization ;
    foaf:name "University of Koblenz" .

_:org-vienna-university-of-economics-and-business a foaf:Organization ;
    foaf:name "Vienna University of Economics and Business" .

_:org-vienna-university-of-technology a foaf:Organization ;
    foaf:name "Vienna University of Technology" .

_:b3f250dcd774fd0efbd1543bc5def1d0b a schema:WebPage ;
    schema:name "IEC 31010:2019" ;
    schema:url "https://www.iso.org/standard/72140.html" .

_:b89b5ee884952f33d70d4fddc4220b465 a schema:WebPage ;
    schema:name "ENISA Threat Landscape for Ransomware Attacks 2022" ;
    schema:url "https://www.enisa.europa.eu/publications/enisa-threat-landscape-for-ransomware-attacks" .

_:org-adapt-centre-trinity-college-dublin a foaf:Organization ;
    foaf:name "ADAPT Centre, Trinity College Dublin" .

_:person-axel-polleres a dct:Agent,
        foaf:Person ;
    org:memberOf _:org-vienna-university-of-economics-and-business ;
    foaf:name "Axel Polleres" .

_:person-julio-hernandez a dct:Agent,
        foaf:Person ;
    org:memberOf _:org-dublin-city-university ;
    foaf:name "Julio Hernandez" .

_:person-fajar-ekaputra a dct:Agent,
        foaf:Person ;
    org:memberOf _:org-vienna-university-of-technology ;
    foaf:name "Fajar Ekaputra" .

_:person-rob-brennan a dct:Agent,
        foaf:Person ;
    scoro:hasORCID "0000-0001-8236-362X" ;
    org:memberOf _:org-university-college-dublin ;
    foaf:name "Rob Brennan" .

_:b65de0d403668931587d7f38d790f5adc a schema:WebPage ;
    schema:name "ENISA Threat Taxonomy 2016" ;
    schema:url "https://www.enisa.europa.eu/topics/threat-risk-management/threats-and-trends/enisa-threat-landscape/threat-taxonomy/view" .

_:person-beatriz-esteves a dct:Agent,
        foaf:Person ;
    scoro:hasORCID "0000-0003-0259-7560" ;
    org:memberOf _:org-idlab-imec-ghent-university ;
    foaf:homepage "https://w3id.org/people/besteves" ;
    foaf:name "Beatriz Esteves" .

_:person-julian-flake a dct:Agent,
        foaf:Person ;
    scoro:hasORCID "0009-0006-4623-1463" ;
    org:memberOf _:org-university-of-koblenz ;
    foaf:name "Julian Flake" .

_:bba19dc259a53f0cb59375372938fbb0a a schema:WebPage ;
    schema:name "ENISA Methodology for Sectoral Cybersecurity Assessments" ;
    schema:url "https://www.enisa.europa.eu/publications/methodology-for-a-sectoral-cybersecurity-assessment" .

_:person-arthit-suriyawongkul a dct:Agent,
        foaf:Person ;
    scoro:hasORCID "0000-0002-9698-1899" ;
    org:memberOf _:org-adapt-centre-trinity-college-dublin ;
    foaf:name "Arthit Suriyawongkul" .

_:person-georg-p-krog a dct:Agent,
        foaf:Person ;
    org:memberOf _:org-signatu-as ;
    foaf:homepage "https://www.linkedin.com/in/georg-philip-krog-a2a278104/" ;
    foaf:name "Georg P. Krog" .

_:b7191aa21b975cb14bbce32aa3ba9c7eb a schema:WebPage ;
    schema:name "ENISA Reference Incident Classification Taxonomy 2018" ;
    schema:url "https://www.enisa.europa.eu/publications/reference-incident-classification-taxonomy/" .

_:person-daniel-doherty a dct:Agent,
        foaf:Person ;
    org:memberOf _:org-trinity-college-dublin ;
    foaf:name "Daniel Doherty" .

_:b15886bc6e88dcdb258fe59ded7be3abf a schema:WebPage ;
    schema:name "ISO/IEC 27005:2018" ;
    schema:url "https://www.iso.org/standard/75281.html" .

_:person-delaram-golpayegani a dct:Agent,
        foaf:Person ;
    scoro:hasORCID "0000-0002-1208-186X" ;
    org:memberOf _:org-adapt-centre-trinity-college-dublin ;
    foaf:name "Delaram Golpayegani" .

_:person-harshvardhan-j-pandit a dct:Agent,
        foaf:Person ;
    scoro:hasORCID "0000-0002-5068-3714" ;
    org:memberOf _:org-ai-accountability-lab-aial-trinity-college-dublin ;
    foaf:homepage "https://harshp.com/" ;
    foaf:name "Harshvardhan J. Pandit" .

