@prefix bibo: <http://purl.org/ontology/bibo/> .
@prefix dct: <http://purl.org/dc/terms/> .
@prefix dpv: <https://w3id.org/dpv#> .
@prefix foaf: <http://xmlns.com/foaf/0.1/> .
@prefix org: <http://www.w3.org/ns/org#> .
@prefix owl: <http://www.w3.org/2002/07/owl#> .
@prefix profile: <http://www.w3.org/ns/dx/prof/> .
@prefix rdf: <http://www.w3.org/1999/02/22-rdf-syntax-ns#> .
@prefix rdfs: <http://www.w3.org/2000/01/rdf-schema#> .
@prefix role: <http://www.w3.org/ns/dx/prof/role/> .
@prefix schema: <https://schema.org/> .
@prefix scoro: <http://purl.org/spar/scoro/> .
@prefix sector-finance: <https://w3id.org/dpv/sector/finance#> .
@prefix skos: <http://www.w3.org/2004/02/skos/core#> .
@prefix sw: <http://www.w3.org/2003/06/sw-vocab-status/ns#> .
@prefix vann: <http://purl.org/vocab/vann/> .
@prefix xsd: <http://www.w3.org/2001/XMLSchema#> .

sector-finance:AccountManagement a rdfs:Class,
        skos:Concept,
        dpv:Purpose ;
    dct:created "2024-12-01"^^xsd:date ;
    rdfs:isDefinedBy sector-finance: ;
    sw:term_status "accepted"@en ;
    skos:broader sector-finance:ServiceProvision ;
    skos:definition "Purposes associated with management of accounts in relation to financial services"@en ;
    skos:inScheme sector-finance:purposes-classes ;
    skos:prefLabel "Account Management"@en .

sector-finance:AntiMoneyLaunderingCompliance a rdfs:Class,
        skos:Concept,
        dpv:Purpose ;
    dct:created "2024-12-01"^^xsd:date ;
    rdfs:isDefinedBy sector-finance: ;
    sw:term_status "accepted"@en ;
    skos:broader sector-finance:AntiMoneyLaunderingManagement,
        sector-finance:RegulatoryCompliance ;
    skos:definition "Purposes associated with compliance assessment, documentation, and reporting activities in relation to anti-money laundering legislations for financial services"@en ;
    skos:inScheme sector-finance:purposes-classes ;
    skos:prefLabel "Anti Money Laundering Compliance"@en .

sector-finance:AntiMoneyLaunderingManagement a rdfs:Class,
        skos:Concept,
        dpv:Purpose ;
    dct:created "2024-12-01"^^xsd:date ;
    rdfs:isDefinedBy sector-finance: ;
    sw:term_status "accepted"@en ;
    skos:broader sector-finance:FraudManagement ;
    skos:definition "Purposes associated with discovery, handling, prediction, and assessment of anti-money laundering activities in relation to financial services"@en ;
    skos:inScheme sector-finance:purposes-classes ;
    skos:prefLabel "Anti-Money Laundering Management"@en .

sector-finance:BudgetPlanningAssistance a rdfs:Class,
        skos:Concept,
        dpv:Purpose ;
    dct:created "2024-12-01"^^xsd:date ;
    rdfs:isDefinedBy sector-finance: ;
    sw:term_status "accepted"@en ;
    skos:broader sector-finance:ServiceProvision ;
    skos:definition "Purposes associated with planning of budgets, spending, and related activities in relation to financial services"@en ;
    skos:inScheme sector-finance:purposes-classes ;
    skos:prefLabel "Budget Planning Assistance"@en .

sector-finance:CreditChecking a rdfs:Class,
        skos:Concept,
        dpv:Purpose ;
    dct:contributor _:N0a43dd9ea5e94fe695d8b7df8802cfdd ;
    dct:created "2022-04-20"^^xsd:date ;
    dct:modified "2024-12-01"^^xsd:date ;
    rdfs:isDefinedBy sector-finance: ;
    sw:term_status "modified"@en ;
    skos:broader sector-finance:FinancialServiceManagement ;
    skos:definition "Purposes associated with maintaining, evaluating, and related activities in relation to calculation of credit scores and related metrics within financial services"@en ;
    skos:inScheme sector-finance:purposes-classes ;
    skos:prefLabel "Credit Checking"@en .

sector-finance:CreditHistoryEvaluation a rdfs:Class,
        skos:Concept,
        dpv:Purpose ;
    dct:created "2024-12-01"^^xsd:date ;
    rdfs:isDefinedBy sector-finance: ;
    sw:term_status "accepted"@en ;
    skos:broader sector-finance:CreditChecking ;
    skos:definition "Purposes associated with evaluation and assessment of credit history in relation to financial services"@en ;
    skos:inScheme sector-finance:purposes-classes ;
    skos:prefLabel "Credit History Evaluation"@en .

sector-finance:CreditLimitDetermination a rdfs:Class,
        skos:Concept,
        dpv:Purpose ;
    dct:created "2024-12-01"^^xsd:date ;
    rdfs:isDefinedBy sector-finance: ;
    sw:term_status "accepted"@en ;
    skos:broader sector-finance:CreditChecking ;
    skos:definition "Purposes associated with determination and calculation of credit limits in relation to financial services"@en ;
    skos:inScheme sector-finance:purposes-classes ;
    skos:prefLabel "Credit Limit Determination"@en .

sector-finance:CreditScoreEvaluation a rdfs:Class,
        skos:Concept,
        dpv:Purpose ;
    dct:created "2024-12-01"^^xsd:date ;
    rdfs:isDefinedBy sector-finance: ;
    sw:term_status "accepted"@en ;
    skos:broader sector-finance:CreditChecking ;
    skos:definition "Purposes associated with evaluation and calculation of credit scores in relation to financial services"@en ;
    skos:inScheme sector-finance:purposes-classes ;
    skos:prefLabel "Credit Score Evaluation"@en .

sector-finance:CustomerDueDiligence a rdfs:Class,
        skos:Concept,
        dpv:Purpose ;
    dct:created "2024-12-01"^^xsd:date ;
    rdfs:isDefinedBy sector-finance: ;
    sw:term_status "accepted"@en ;
    skos:broader sector-finance:RegulatoryCompliance ;
    skos:definition "Purposes associated with compliance assessment, documentation, and reporting activities in relation to customer due diligence legislations for financial services"@en ;
    skos:inScheme sector-finance:purposes-classes ;
    skos:prefLabel "Customer Due Diligence"@en .

sector-finance:DebtManagement a rdfs:Class,
        skos:Concept,
        dpv:Purpose ;
    dct:created "2024-12-01"^^xsd:date ;
    rdfs:isDefinedBy sector-finance: ;
    sw:term_status "accepted"@en ;
    skos:broader sector-finance:ServiceProvision ;
    skos:definition "Purposes associated with management of debt in relation to financial services"@en ;
    skos:inScheme sector-finance:purposes-classes ;
    skos:prefLabel "Debt Management"@en .

sector-finance:ExpenseManagement a rdfs:Class,
        skos:Concept,
        dpv:Purpose ;
    dct:created "2024-12-01"^^xsd:date ;
    rdfs:isDefinedBy sector-finance: ;
    sw:term_status "accepted"@en ;
    skos:broader sector-finance:ServiceProvision ;
    skos:definition "Purposes associated with management of expenses and related activities in relation to financial services"@en ;
    skos:inScheme sector-finance:purposes-classes ;
    skos:prefLabel "Expense Management"@en .

sector-finance:FinancialServiceManagement a rdfs:Class,
        skos:Concept,
        dpv:Purpose ;
    dct:created "2024-12-01"^^xsd:date ;
    rdfs:isDefinedBy sector-finance: ;
    sw:term_status "accepted"@en ;
    skos:broader dpv:Purpose ;
    skos:definition "Purposes associated with management of financial services"@en ;
    skos:inScheme sector-finance:purposes-classes ;
    skos:prefLabel "Financial Service Management"@en .

sector-finance:FraudManagement a rdfs:Class,
        skos:Concept,
        dpv:Purpose ;
    dct:created "2024-12-01"^^xsd:date ;
    rdfs:isDefinedBy sector-finance: ;
    sw:term_status "accepted"@en ;
    skos:broader dpv:FraudPreventionAndDetection,
        sector-finance:FinancialServiceManagement ;
    skos:definition "Purposes associated with management of fraud, including fraud prevention and detection, in relation to financial services"@en ;
    skos:inScheme sector-finance:purposes-classes ;
    skos:prefLabel "Fraud Management"@en .

sector-finance:IdentityFraudManagement a rdfs:Class,
        skos:Concept,
        dpv:Purpose ;
    dct:created "2024-12-01"^^xsd:date ;
    rdfs:isDefinedBy sector-finance: ;
    sw:term_status "accepted"@en ;
    skos:broader sector-finance:FraudManagement ;
    skos:definition "Purposes associated with discovery, handling, prediction, and assessment of identity frauds in relation to financial services"@en ;
    skos:inScheme sector-finance:purposes-classes ;
    skos:prefLabel "Identity Fraud Management"@en .

sector-finance:InstabilityRiskAssessment a rdfs:Class,
        skos:Concept,
        dpv:Purpose ;
    dct:created "2024-12-01"^^xsd:date ;
    rdfs:isDefinedBy sector-finance: ;
    sw:term_status "accepted"@en ;
    skos:broader sector-finance:CreditChecking ;
    skos:definition "Purposes associated with financial instability risk assessments in relation to financial services"@en ;
    skos:inScheme sector-finance:purposes-classes ;
    skos:prefLabel "Instability Risk Assessment"@en .

sector-finance:InsuranceClaimDisputeResolution a rdfs:Class,
        skos:Concept,
        dpv:Purpose ;
    dct:created "2024-12-01"^^xsd:date ;
    rdfs:isDefinedBy sector-finance: ;
    sw:term_status "accepted"@en ;
    skos:broader sector-finance:InsuranceClaimsManagement ;
    skos:definition "Purposes associated with dispute resolution regarding insurnace claims"@en ;
    skos:inScheme sector-finance:purposes-classes ;
    skos:prefLabel "Insurance Claim Dispute Resolution"@en .

sector-finance:InsuranceClaimEligibilityAssessment a rdfs:Class,
        skos:Concept,
        dpv:Purpose ;
    dct:created "2024-12-01"^^xsd:date ;
    rdfs:isDefinedBy sector-finance: ;
    sw:term_status "accepted"@en ;
    skos:broader dpv:FraudPreventionAndDetection,
        sector-finance:InsuranceClaimsManagement ;
    skos:definition "Purposes associated with assessing the eligibility of insurance claims"@en ;
    skos:inScheme sector-finance:purposes-classes ;
    skos:prefLabel "Insurance Claim Eligibility Assessment"@en .

sector-finance:InsuranceClaimFraudManagement a rdfs:Class,
        skos:Concept,
        dpv:Purpose ;
    dct:created "2024-12-01"^^xsd:date ;
    rdfs:isDefinedBy sector-finance: ;
    sw:term_status "accepted"@en ;
    skos:broader sector-finance:InsuranceClaimsManagement,
        sector-finance:InsuranceFraudManagement ;
    skos:definition "Purposes associated with fraud prevention and detection related to insurnace claims"@en ;
    skos:inScheme sector-finance:purposes-classes ;
    skos:prefLabel "Insurance Claim Fraud Management"@en .

sector-finance:InsuranceClaimPayoutAssessment a rdfs:Class,
        skos:Concept,
        dpv:Purpose ;
    dct:created "2024-12-01"^^xsd:date ;
    rdfs:isDefinedBy sector-finance: ;
    sw:term_status "accepted"@en ;
    skos:broader sector-finance:InsuranceClaimsManagement ;
    skos:definition "Purposes associated with assessing the amount, validity, and method for payout of insurance claims"@en ;
    skos:inScheme sector-finance:purposes-classes ;
    skos:prefLabel "Insurance Claim Payout Assessment"@en .

sector-finance:InsuranceClaimsManagement a rdfs:Class,
        skos:Concept,
        dpv:Purpose ;
    dct:created "2024-12-01"^^xsd:date ;
    rdfs:isDefinedBy sector-finance: ;
    sw:term_status "accepted"@en ;
    skos:broader sector-finance:InsuranceManagement ;
    skos:definition "Purposes associated with management of insurance claims"@en ;
    skos:inScheme sector-finance:purposes-classes ;
    skos:prefLabel "Insurance Claims Management"@en .

sector-finance:InsuranceCoverageAssessment a rdfs:Class,
        skos:Concept,
        dpv:Purpose ;
    dct:created "2024-12-01"^^xsd:date ;
    rdfs:isDefinedBy sector-finance: ;
    sw:term_status "accepted"@en ;
    skos:broader sector-finance:InsuranceManagement ;
    skos:definition "Purposes associated with assessing the validity of existing insurance coverage for specific situations and contexts"@en ;
    skos:inScheme sector-finance:purposes-classes ;
    skos:prefLabel "Insurance Coverage Assessment"@en .

sector-finance:InsuranceEligibilityAssessment a rdfs:Class,
        skos:Concept,
        dpv:Purpose ;
    dct:created "2024-12-01"^^xsd:date ;
    rdfs:isDefinedBy sector-finance: ;
    sw:term_status "accepted"@en ;
    skos:broader sector-finance:InsuranceManagement ;
    skos:definition "Purposes associated with assessment of elibility for receiving or continuing to receive insurance"@en ;
    skos:inScheme sector-finance:purposes-classes ;
    skos:prefLabel "Insurance Eligibility Assessment"@en .

sector-finance:InsuranceFraudManagement a rdfs:Class,
        skos:Concept,
        dpv:Purpose ;
    dct:created "2024-12-01"^^xsd:date ;
    rdfs:isDefinedBy sector-finance: ;
    sw:term_status "accepted"@en ;
    skos:broader dpv:FraudPreventionAndDetection,
        sector-finance:InsuranceManagement ;
    skos:definition "Purposes associated with fraud prevention and detection related to insurance"@en ;
    skos:inScheme sector-finance:purposes-classes ;
    skos:prefLabel "Insurance Fraud Management"@en .

sector-finance:InsuranceIdentityFraudManagement a rdfs:Class,
        skos:Concept,
        dpv:Purpose ;
    dct:created "2024-12-01"^^xsd:date ;
    rdfs:isDefinedBy sector-finance: ;
    sw:term_status "accepted"@en ;
    skos:broader sector-finance:InsuranceFraudManagement ;
    skos:definition "Purposes associated with identity fraud prevention and detection related to insurance"@en ;
    skos:inScheme sector-finance:purposes-classes ;
    skos:prefLabel "Insurance Identity Fraud Management"@en .

sector-finance:InsuranceManagement a rdfs:Class,
        skos:Concept,
        dpv:Purpose ;
    dct:created "2024-12-01"^^xsd:date ;
    rdfs:isDefinedBy sector-finance: ;
    sw:term_status "accepted"@en ;
    skos:broader dpv:Purpose ;
    skos:definition "Purposes associated with management of insurance"@en ;
    skos:inScheme sector-finance:purposes-classes ;
    skos:prefLabel "Insurance Management"@en .

sector-finance:InsurancePersonalisedPricingManagement a rdfs:Class,
        skos:Concept,
        dpv:Purpose ;
    dct:created "2024-12-01"^^xsd:date ;
    rdfs:isDefinedBy sector-finance: ;
    sw:term_status "accepted"@en ;
    skos:broader dpv:ServicePersonalisation,
        sector-finance:InsuranceManagement ;
    skos:definition "Purposes associated with the use of personalisation in determination, optimisation, and other processes related to pricing of insurance premiums"@en ;
    skos:inScheme sector-finance:purposes-classes ;
    skos:prefLabel "Insurance Personalised Pricing Management"@en .

sector-finance:InsurancePricingManagement a rdfs:Class,
        skos:Concept,
        dpv:Purpose ;
    dct:created "2024-12-01"^^xsd:date ;
    rdfs:isDefinedBy sector-finance: ;
    sw:term_status "accepted"@en ;
    skos:broader sector-finance:InsuranceManagement ;
    skos:definition "Purposes associated with determination, optimisation, and other processes related to pricing of insurance premiums"@en ;
    skos:inScheme sector-finance:purposes-classes ;
    skos:prefLabel "Insurance Pricing Management"@en .

sector-finance:InsuranceRiskAssessment a rdfs:Class,
        skos:Concept,
        dpv:Purpose ;
    dct:created "2024-12-01"^^xsd:date ;
    rdfs:isDefinedBy sector-finance: ;
    sw:term_status "accepted"@en ;
    skos:broader dpv:FraudPreventionAndDetection,
        sector-finance:InsuranceManagement ;
    skos:definition "Purposes associated with conducting risk assessments in the context of insurance services"@en ;
    skos:inScheme sector-finance:purposes-classes ;
    skos:prefLabel "Insurance Risk Assessment"@en .

sector-finance:InvestmentManagement a rdfs:Class,
        skos:Concept,
        dpv:Purpose ;
    dct:created "2024-12-01"^^xsd:date ;
    rdfs:isDefinedBy sector-finance: ;
    sw:term_status "accepted"@en ;
    skos:broader sector-finance:ServiceProvision ;
    skos:definition "Purposes associated with management of investments, portfolios, and related activities as part of financial services"@en ;
    skos:inScheme sector-finance:purposes-classes ;
    skos:prefLabel "Investment Management"@en .

sector-finance:LoanServiceProvision a rdfs:Class,
        skos:Concept,
        dpv:Purpose ;
    dct:created "2024-12-01"^^xsd:date ;
    rdfs:isDefinedBy sector-finance: ;
    sw:term_status "accepted"@en ;
    skos:broader sector-finance:ServiceProvision ;
    skos:definition "Purposes associated with provision of loans and related activities in relation to financial services"@en ;
    skos:inScheme sector-finance:purposes-classes ;
    skos:prefLabel "Loan Service Provision"@en .

sector-finance:MaintainCreditCheckingDatabase a rdfs:Class,
        skos:Concept,
        dpv:Purpose ;
    dct:contributor _:N05cd1f43dbaf4b4ba297dab5ee221394,
        _:N0a43dd9ea5e94fe695d8b7df8802cfdd ;
    dct:created "2022-06-15"^^xsd:date ;
    dct:modified "2024-12-01"^^xsd:date ;
    rdfs:isDefinedBy sector-finance: ;
    sw:term_status "modified"@en ;
    skos:broader sector-finance:CreditChecking ;
    skos:definition "Purposes associated with maintaining a Credit Checking Database"@en ;
    skos:inScheme sector-finance:purposes-classes ;
    skos:prefLabel "Maintain Credit Checking Database"@en .

sector-finance:MaintainCreditRatingDatabase a rdfs:Class,
        skos:Concept,
        dpv:Purpose ;
    dct:contributor _:N05cd1f43dbaf4b4ba297dab5ee221394,
        _:N0a43dd9ea5e94fe695d8b7df8802cfdd ;
    dct:created "2022-06-15"^^xsd:date ;
    dct:modified "2024-12-01"^^xsd:date ;
    rdfs:isDefinedBy sector-finance: ;
    sw:term_status "modified"@en ;
    skos:broader sector-finance:CreditChecking ;
    skos:definition "Purposes associated with maintaining a Credit Rating Database"@en ;
    skos:inScheme sector-finance:purposes-classes ;
    skos:prefLabel "Maintain Credit Rating Database"@en .

sector-finance:PaymentProcessing a rdfs:Class,
        skos:Concept,
        dpv:Purpose ;
    dct:created "2024-12-01"^^xsd:date ;
    rdfs:isDefinedBy sector-finance: ;
    sw:term_status "accepted"@en ;
    skos:broader sector-finance:ServiceProvision ;
    skos:definition "Purposes associated with payment processing and related payment activities in relation to financial services"@en ;
    skos:inScheme sector-finance:purposes-classes ;
    skos:prefLabel "Payment Processing"@en .

sector-finance:PersonalisedServiceProvision a rdfs:Class,
        skos:Concept,
        dpv:Purpose ;
    dct:created "2024-12-01"^^xsd:date ;
    rdfs:isDefinedBy sector-finance: ;
    sw:term_status "accepted"@en ;
    skos:broader dpv:ServicePersonalisation,
        sector-finance:FinancialServiceManagement ;
    skos:definition "Purposes associated with providing personalised financial services"@en ;
    skos:inScheme sector-finance:purposes-classes ;
    skos:prefLabel "Personalised Service Provision"@en .

sector-finance:PhishingAttackManagement a rdfs:Class,
        skos:Concept,
        dpv:Purpose ;
    dct:created "2024-12-01"^^xsd:date ;
    rdfs:isDefinedBy sector-finance: ;
    sw:term_status "accepted"@en ;
    skos:broader sector-finance:FraudManagement ;
    skos:definition "Purposes associated with discovery, handling, prediction, and assessment of phishing attacks in relation to financial services"@en ;
    skos:inScheme sector-finance:purposes-classes ;
    skos:prefLabel "Phishing Attack Management"@en .

sector-finance:ProductRecommendation a rdfs:Class,
        skos:Concept,
        dpv:Purpose ;
    dct:created "2024-12-01"^^xsd:date ;
    rdfs:isDefinedBy sector-finance: ;
    sw:term_status "accepted"@en ;
    skos:broader sector-finance:ServiceProvision ;
    skos:definition "Purposes associated with providing product recommendations as part of financial services"@en ;
    skos:inScheme sector-finance:purposes-classes ;
    skos:prefLabel "Product Recommendation"@en .

sector-finance:RegulatoryCompliance a rdfs:Class,
        skos:Concept,
        dpv:Purpose ;
    dct:created "2024-12-01"^^xsd:date ;
    rdfs:isDefinedBy sector-finance: ;
    sw:term_status "accepted"@en ;
    skos:broader dpv:LegalCompliance,
        sector-finance:FinancialServiceManagement ;
    skos:definition "Purposes associated with regulatory compliance assessment, documentation, and reporting activities in relation to financial services"@en ;
    skos:inScheme sector-finance:purposes-classes ;
    skos:prefLabel "Regulatory Compliance"@en .

sector-finance:ServiceImprovement a rdfs:Class,
        skos:Concept,
        dpv:Purpose ;
    dct:created "2024-12-01"^^xsd:date ;
    rdfs:isDefinedBy sector-finance: ;
    sw:term_status "accepted"@en ;
    skos:broader dpv:ServiceOptimisation,
        sector-finance:FinancialServiceManagement ;
    skos:definition "Purposes associated with identifying, planning, and carrying out improvements to financial services"@en ;
    skos:inScheme sector-finance:purposes-classes ;
    skos:prefLabel "Service Improvement"@en .

sector-finance:ServiceProvision a rdfs:Class,
        skos:Concept,
        dpv:Purpose ;
    dct:created "2024-12-01"^^xsd:date ;
    rdfs:isDefinedBy sector-finance: ;
    sw:term_status "accepted"@en ;
    skos:broader dpv:ServiceProvision,
        sector-finance:FinancialServiceManagement ;
    skos:definition "Purposes associated with provision of financial services"@en ;
    skos:inScheme sector-finance:purposes-classes ;
    skos:prefLabel "Service Provision"@en .

sector-finance:TaxReportingCompliance a rdfs:Class,
        skos:Concept,
        dpv:Purpose ;
    dct:created "2024-12-01"^^xsd:date ;
    rdfs:isDefinedBy sector-finance: ;
    sw:term_status "accepted"@en ;
    skos:broader sector-finance:RegulatoryCompliance ;
    skos:definition "Purposes associated with compliance assessment, documentation, and reporting activities in relation to taxation legislations for financial services"@en ;
    skos:inScheme sector-finance:purposes-classes ;
    skos:prefLabel "Tax Reporting Compliance"@en .

sector-finance:TransactionFraudManagement a rdfs:Class,
        skos:Concept,
        dpv:Purpose ;
    dct:created "2024-12-01"^^xsd:date ;
    rdfs:isDefinedBy sector-finance: ;
    sw:term_status "accepted"@en ;
    skos:broader sector-finance:FraudManagement ;
    skos:definition "Purposes associated with discovery, handling, prediction, and assessment of transaction frauds in relation to financial services"@en ;
    skos:inScheme sector-finance:purposes-classes ;
    skos:prefLabel "Transaction Fraud Management"@en .

sector-finance:TransactionReportingCompliance a rdfs:Class,
        skos:Concept,
        dpv:Purpose ;
    dct:created "2024-12-01"^^xsd:date ;
    rdfs:isDefinedBy sector-finance: ;
    sw:term_status "accepted"@en ;
    skos:broader sector-finance:RegulatoryCompliance ;
    skos:definition "Purposes associated with compliance assessment, documentation, and reporting activities in relation to transaction reporting legislations for financial services"@en ;
    skos:inScheme sector-finance:purposes-classes ;
    skos:prefLabel "Transaction Reporting Compliance"@en .

sector-finance:WealthManagement a rdfs:Class,
        skos:Concept,
        dpv:Purpose ;
    dct:created "2024-12-01"^^xsd:date ;
    rdfs:isDefinedBy sector-finance: ;
    sw:term_status "accepted"@en ;
    skos:broader sector-finance:ServiceProvision ;
    skos:definition "Purposes associated with wealth management in relation to financial services"@en ;
    skos:inScheme sector-finance:purposes-classes ;
    skos:prefLabel "Wealth Management"@en .

<https://w3id.org/dpv/sector/finance> a owl:Ontology,
        profile:Profile ;
    dct:bibliographicCitation "Harshvardhan J. Pandit, Beatriz Esteves, Georg P. Krog, Paul Ryan, Delaram Golpayegani, Julian Flake (2025) Data Privacy Vocabulary (DPV) – Version 2.0. In: Demartini, G., et al. The Semantic Web – ISWC 2024. ISWC 2024. Lecture Notes in Computer Science, vol 15233. Springer, Cham. https://doi.org/10.1007/978-3-031-77847-6_10" ;
    dct:conformsTo "http://www.w3.org/2000/01/rdf-schema",
        "http://www.w3.org/2004/02/skos/core" ;
    dct:contributor _:N05cd1f43dbaf4b4ba297dab5ee221394,
        _:N0a43dd9ea5e94fe695d8b7df8802cfdd ;
    dct:created "2024-12-01"@en ;
    dct:creator _:N0a43dd9ea5e94fe695d8b7df8802cfdd ;
    dct:description "Extension to the Data Privacy Vocabulary (DPV) providing concepts for the finance sector"@en ;
    dct:identifier "https://w3id.org/dpv/sector/finance" ;
    dct:issued "2024-12-01"@en ;
    dct:license <https://www.w3.org/copyright/document-license-2023/> ;
    dct:modified "2025-03-16"@en ;
    dct:publisher <https://www.w3.org/> ;
    dct:source <https://www.w3.org/groups/cg/dpvcg/> ;
    dct:title "Finance Sector Concepts"@en ;
    bibo:doi "10.5281/zenodo.12505841" ;
    bibo:status "http://purl.org/ontology/bibo/status/draft" ;
    vann:preferredNamespacePrefix "sector-finance" ;
    vann:preferredNamespaceUri "https://w3id.org/dpv/sector/finance#" ;
    rdfs:Label "SECTOR-FINANCE"@en ;
    owl:versionIRI <https://w3id.org/dpv/2.1/sector/finance> ;
    owl:versionInfo "2.1" ;
    profile:hasResource <https://w3id.org/dpv/examples>,
        <https://w3id.org/dpv/guides>,
        <https://w3id.org/dpv/primer>,
        sector-finance:serialisation-html,
        sector-finance:serialisation-jsonld,
        sector-finance:serialisation-n3,
        sector-finance:serialisation-rdf,
        sector-finance:serialisation-ttl ;
    profile:isProfileOf rdfs:,
        skos:,
        <https://w3id.org/dpv> ;
    foaf:logo <https://w3id.org/dpv/media/logo.png> ;
    schema:version "2.1" .

sector-finance:serialisation-html a profile:ResourceDescriptor ;
    dct:conformsTo <https://www.w3.org/TR/html/> ;
    dct:format <https://www.iana.org/assignments/media-types/text/html> ;
    dct:title "Finance Sector Concepts - HTML serialiation" ;
    profile:hasArtifact <https://w3id.org/dpv/sector/finance/sector-finance.html> ;
    profile:hasRole role:specification .

sector-finance:serialisation-jsonld a profile:ResourceDescriptor ;
    dct:conformsTo <https://www.w3.org/TR/json-ld11/> ;
    dct:format <https://www.iana.org/assignments/media-types/application/ld+json> ;
    dct:title "Finance Sector Concepts - JSON-LD serialiation" ;
    profile:hasArtifact <https://w3id.org/dpv/sector/finance/sector-finance.jsonld> ;
    profile:hasRole role:vocabulary .

sector-finance:serialisation-n3 a profile:ResourceDescriptor ;
    dct:conformsTo <https://www.w3.org/TeamSubmission/n3/> ;
    dct:format <https://www.iana.org/assignments/media-types/text/n3> ;
    dct:title "Finance Sector Concepts - N3 serialiation" ;
    profile:hasArtifact <https://w3id.org/dpv/sector/finance/sector-finance.n3> ;
    profile:hasRole role:vocabulary .

sector-finance:serialisation-rdf a profile:ResourceDescriptor ;
    dct:conformsTo rdf: ;
    dct:format <https://www.iana.org/assignments/media-types/application/rdf+xml> ;
    dct:title "Finance Sector Concepts - RDF/XML serialiation" ;
    profile:hasArtifact <https://w3id.org/dpv/sector/finance/sector-finance.rdf> ;
    profile:hasRole role:vocabulary .

sector-finance:serialisation-ttl a profile:ResourceDescriptor ;
    dct:conformsTo <https://www.w3.org/TR/turtle/> ;
    dct:format <https://www.iana.org/assignments/media-types/text/turtle> ;
    dct:title "Finance Sector Concepts - Turtle serialiation" ;
    profile:hasArtifact <https://w3id.org/dpv/sector/finance/sector-finance.ttl> ;
    profile:hasRole role:vocabulary .

<https://w3id.org/dpv/examples> a profile:ResourceDescriptor ;
    dct:conformsTo <https://www.w3.org/TR/html/> ;
    dct:format <https://www.iana.org/assignments/media-types/text/html> ;
    dct:title "Examples for Data Privacy Vocabulary" ;
    profile:hasArtifact <https://w3id.org/dpv/examples> ;
    profile:hasRole role:guidance .

<https://w3id.org/dpv/guides> a profile:ResourceDescriptor ;
    dct:conformsTo <https://www.w3.org/TR/html/> ;
    dct:format <https://www.iana.org/assignments/media-types/text/html> ;
    dct:title "Guides for Data Privacy Vocabulary" ;
    profile:hasArtifact <https://w3id.org/dpv/guides> ;
    profile:hasRole role:guidance .

<https://w3id.org/dpv/primer> a profile:ResourceDescriptor ;
    dct:conformsTo <https://www.w3.org/TR/html/> ;
    dct:format <https://www.iana.org/assignments/media-types/text/html> ;
    dct:title "Primer for Data Privacy Vocabulary" ;
    profile:hasArtifact <https://w3id.org/dpv/primer> ;
    profile:hasRole role:guidance .

sector-finance:purposes-classes a skos:ConceptScheme .

_:N2bfb2dfcc0b24c5182bd06c242c085fa a foaf:Organization ;
    foaf:name "Signatu AS" .

_:N313d89a6c37147bfac1bbb4aa7f6510b a foaf:Organization ;
    foaf:name "ADAPT Centre, Dublin City University" .

_:N05cd1f43dbaf4b4ba297dab5ee221394 a dct:Agent,
        foaf:Person ;
    org:memberOf _:N2bfb2dfcc0b24c5182bd06c242c085fa ;
    foaf:homepage "https://www.linkedin.com/in/georg-philip-krog-a2a278104/" ;
    foaf:name "Georg P. Krog" .

_:N0a43dd9ea5e94fe695d8b7df8802cfdd a dct:Agent,
        foaf:Person ;
    scoro:hasORCID "0000-0002-5068-3714" ;
    org:memberOf _:N313d89a6c37147bfac1bbb4aa7f6510b ;
    foaf:homepage "https://harshp.com/" ;
    foaf:name "Harshvardhan J. Pandit" .

