@prefix ai-owl: <https://w3id.org/dpv/ai/owl#> .
@prefix bibo: <http://purl.org/ontology/bibo/> .
@prefix dcam: <http://purl.org/dc/dcam/> .
@prefix dct: <http://purl.org/dc/terms/> .
@prefix dpv-owl: <https://w3id.org/dpv/owl#> .
@prefix foaf: <http://xmlns.com/foaf/0.1/> .
@prefix org: <http://www.w3.org/ns/org#> .
@prefix owl: <http://www.w3.org/2002/07/owl#> .
@prefix profile: <http://www.w3.org/ns/dx/prof/> .
@prefix rdf: <http://www.w3.org/1999/02/22-rdf-syntax-ns#> .
@prefix rdfs: <http://www.w3.org/2000/01/rdf-schema#> .
@prefix risk-owl: <https://w3id.org/dpv/risk/owl#> .
@prefix role: <http://www.w3.org/ns/dx/prof/role/> .
@prefix schema: <https://schema.org/> .
@prefix scoro: <http://purl.org/spar/scoro/> .
@prefix skos: <http://www.w3.org/2004/02/skos/core#> .
@prefix sw: <http://www.w3.org/2003/06/sw-vocab-status/ns#> .
@prefix tech-owl: <https://w3id.org/dpv/tech/owl#> .
@prefix vann: <http://purl.org/vocab/vann/> .
@prefix xsd: <http://www.w3.org/2001/XMLSchema#> .

ai-owl:AGI a rdfs:Class,
        owl:Class ;
    dct:contributor _:Ne8d6151e3d8047e6a947b3ec1a3830a1 ;
    dct:created "2024-12-01"^^xsd:date ;
    dct:source "ISO/IEC 22989:2022"@en ;
    rdfs:isDefinedBy ai-owl: ;
    rdfs:subClassOf ai-owl:AISystem ;
    sw:term_status "accepted"@en ;
    skos:definition "Type of AI system that addresses a broad range of tasks with a satisfactory level of performance"@en ;
    skos:prefLabel "Artificial General Intelligence (AGI)"@en .

ai-owl:AI a rdfs:Class,
        owl:Class ;
    dct:contributor _:Ne8d6151e3d8047e6a947b3ec1a3830a1 ;
    dct:created "2024-04-28"^^xsd:date ;
    dct:source "ISO/IEC 22989:2022"@en ;
    rdfs:isDefinedBy ai-owl: ;
    rdfs:subClassOf dpv-owl:Technology ;
    sw:term_status "accepted"@en ;
    skos:definition "A technical and scientific field devoted to the engineered system that generates outputs such as content, forecasts, recommendations or decisions for a given set of human-defined objectives"@en ;
    skos:prefLabel "Artificial Intelligence (AI)"@en .

ai-owl:AIBias a rdfs:Class,
        owl:Class,
        dpv-owl:RiskConcept,
        risk-owl:PotentialRisk,
        risk-owl:PotentialRiskSource ;
    dct:contributor _:N606ea170c32e4fb5ac26e62242d8681b,
        _:Ne8d6151e3d8047e6a947b3ec1a3830a1 ;
    dct:created "2024-09-18"^^xsd:date ;
    rdfs:isDefinedBy ai-owl: ;
    rdfs:subClassOf ai-owl:RiskConcept,
        risk-owl:Bias ;
    sw:term_status "accepted"@en ;
    skos:definition "Bias associated with development, use, or other activities involving an AI technology or system"@en ;
    skos:prefLabel "AI Bias"@en .

ai-owl:AISystem a rdfs:Class,
        owl:Class ;
    dct:contributor _:Ne8d6151e3d8047e6a947b3ec1a3830a1 ;
    dct:created "2024-05-17"^^xsd:date ;
    dct:source " ISO/IEC 22989:2023"@en,
        "OECD.AI"@en ;
    rdfs:isDefinedBy ai-owl: ;
    rdfs:subClassOf ai-owl:AI,
        tech-owl:System ;
    sw:term_status "accepted"@en ;
    skos:definition "An engineered system that generates outputs such as content, forecasts, recommendations or decisions for a given set of human-defined objectives (ISO/IEC 22989:2023 definition); or A machine-based system that, for explicit or implicit objectives, infers, from the input it receives, how to generate outputs such as predictions, content, recommendations, or decisions that can influence physical or virtual environments. Different AI systems vary in their levels of autonomy and adaptiveness after deployment (OECD 2024 definition)"@en ;
    skos:prefLabel "AI System"@en .

ai-owl:AISystemRisk a rdfs:Class,
        owl:Class,
        dpv-owl:RiskConcept,
        risk-owl:PotentialRisk,
        risk-owl:PotentialRiskSource ;
    dct:contributor _:Ne8d6151e3d8047e6a947b3ec1a3830a1 ;
    dct:created "2024-12-01"^^xsd:date ;
    rdfs:isDefinedBy ai-owl: ;
    rdfs:subClassOf ai-owl:RiskConcept ;
    sw:term_status "accepted"@en ;
    skos:definition "Risks associated with AI Systems"@en ;
    skos:prefLabel "AI System Risk"@en .

ai-owl:ActionRecognition a rdfs:Class,
        owl:Class,
        ai-owl:Capability ;
    dct:contributor _:Ne8d6151e3d8047e6a947b3ec1a3830a1 ;
    dct:created "2024-12-01"^^xsd:date ;
    dct:source " Defining Artificial Intelligence 2.0"@en,
        "AI Watch"@en ;
    rdfs:isDefinedBy ai-owl: ;
    rdfs:subClassOf ai-owl:BiometricCapability,
        ai-owl:ComputerVision ;
    sw:term_status "accepted"@en ;
    skos:definition "Capability to recognise actions"@en ;
    skos:prefLabel "Action Recognition"@en .

ai-owl:AdversarialAttack a rdfs:Class,
        owl:Class,
        dpv-owl:RiskConcept,
        risk-owl:IntegrityConcept,
        risk-owl:PotentialConsequence,
        risk-owl:PotentialRisk,
        risk-owl:PotentialRiskSource ;
    dct:contributor _:Ne8d6151e3d8047e6a947b3ec1a3830a1 ;
    dct:created "2024-12-01"^^xsd:date ;
    rdfs:isDefinedBy ai-owl: ;
    rdfs:subClassOf ai-owl:SecurityAttack ;
    sw:term_status "accepted"@en ;
    skos:definition "Inputs designed to cause the model to make a mistake"@en ;
    skos:prefLabel "Adversarial Attack"@en .

ai-owl:AlgorithmSelectionBias a rdfs:Class,
        owl:Class,
        dpv-owl:RiskConcept,
        risk-owl:PotentialRisk,
        risk-owl:PotentialRiskSource ;
    dct:contributor _:N606ea170c32e4fb5ac26e62242d8681b,
        _:Ne8d6151e3d8047e6a947b3ec1a3830a1 ;
    dct:created "2024-09-13"^^xsd:date ;
    dct:source "ISO/IEC 24027:2021"@en ;
    rdfs:isDefinedBy ai-owl: ;
    rdfs:subClassOf ai-owl:EngineeringDecisionBias ;
    sw:term_status "accepted"@en ;
    skos:definition "Bias that occurs from the selection of machine learning algorithms built into the AI system which introduce unwanted bias in predictions made by the system because the type of algorithm used introduces a variation in the performance of the ML model"@en ;
    skos:prefLabel "Algorithm Selection Bias"@en .

ai-owl:AudioCapability a rdfs:Class,
        owl:Class,
        ai-owl:Capability ;
    dct:contributor _:N0a43dd9ea5e94fe695d8b7df8802cfdd ;
    dct:created "2024-12-01"^^xsd:date ;
    rdfs:isDefinedBy ai-owl: ;
    rdfs:subClassOf ai-owl:Capability ;
    sw:term_status "accepted"@en ;
    skos:definition "Capabilities related to the processing and generation of audio"@en ;
    skos:prefLabel "Audio Capability"@en .

ai-owl:AudioGeneration a rdfs:Class,
        owl:Class,
        ai-owl:Capability ;
    dct:contributor _:N0a43dd9ea5e94fe695d8b7df8802cfdd,
        _:Ne8d6151e3d8047e6a947b3ec1a3830a1 ;
    dct:created "2024-12-01"^^xsd:date ;
    rdfs:isDefinedBy ai-owl: ;
    rdfs:subClassOf ai-owl:AudioCapability,
        ai-owl:ContentGeneration ;
    sw:term_status "accepted"@en ;
    skos:definition "Capability to generate audio"@en ;
    skos:prefLabel "Audio Generation"@en .

ai-owl:AudioProcessing a rdfs:Class,
        owl:Class,
        ai-owl:Technique ;
    dct:contributor _:Ne8d6151e3d8047e6a947b3ec1a3830a1 ;
    dct:created "2024-12-01"^^xsd:date ;
    dct:source [ a schema:WebPage ;
            schema:name "AI Watch" ;
            schema:url "Defining Artificial Intelligence 2.0 [https://publications.jrc.ec.europa.eu/repository/handle/JRC126426]" ] ;
    rdfs:isDefinedBy ai-owl: ;
    rdfs:subClassOf ai-owl:Technique ;
    sw:term_status "accepted"@en ;
    skos:definition "Technique involving processing audio"@en ;
    skos:prefLabel "Audio Processing"@en .

ai-owl:AutomaticSummarisation a rdfs:Class,
        owl:Class,
        ai-owl:Capability ;
    dct:contributor _:Ne8d6151e3d8047e6a947b3ec1a3830a1 ;
    dct:created "2024-12-01"^^xsd:date ;
    dct:source " 3.6.1"@en,
        "ISO/IEC 22989:2022"@en ;
    rdfs:isDefinedBy ai-owl: ;
    rdfs:subClassOf ai-owl:InformationRetrieval,
        ai-owl:LanguageCapability ;
    sw:term_status "accepted"@en ;
    skos:definition "Capability for shortening a portion of content such as text while retaining important semantic information"@en ;
    skos:prefLabel "Automatic Summarisation"@en .

ai-owl:AutomationBias a rdfs:Class,
        owl:Class,
        dpv-owl:RiskConcept,
        risk-owl:PotentialRisk,
        risk-owl:PotentialRiskSource ;
    dct:contributor _:N606ea170c32e4fb5ac26e62242d8681b,
        _:Ne8d6151e3d8047e6a947b3ec1a3830a1 ;
    dct:created "2024-09-13"^^xsd:date ;
    dct:source "ISO/IEC 24027:2021"@en ;
    rdfs:isDefinedBy ai-owl: ;
    rdfs:subClassOf ai-owl:AIBias,
        risk-owl:CognitiveBias ;
    sw:term_status "accepted"@en ;
    skos:definition "Bias tha occurs due to propensity for humans to favour suggestions from automated decision-making systems and to ignore contradictory information made without automation, even if it is correct"@en ;
    skos:prefLabel "Automation Bias"@en .

ai-owl:BayesianEstimation a rdfs:Class,
        owl:Class,
        ai-owl:Technique ;
    dct:contributor _:Ne8d6151e3d8047e6a947b3ec1a3830a1 ;
    dct:created "2024-12-01"^^xsd:date ;
    rdfs:isDefinedBy ai-owl: ;
    rdfs:subClassOf ai-owl:StatisticalTechnique ;
    sw:term_status "accepted"@en ;
    skos:definition "Refers to Bayesian estimation approach"@en ;
    skos:prefLabel "Bayesian Estimation"@en .

ai-owl:BayesianNetwork a rdfs:Class,
        owl:Class,
        ai-owl:Technique ;
    dct:contributor _:Ne8d6151e3d8047e6a947b3ec1a3830a1 ;
    dct:created "2024-12-01"^^xsd:date ;
    dct:source " 3.3.1"@en,
        "ISO/IEC 22989"@en ;
    rdfs:isDefinedBy ai-owl: ;
    rdfs:subClassOf ai-owl:StatisticalTechnique ;
    sw:term_status "accepted"@en ;
    skos:definition "Probabilistic technique that uses Bayesian inference for probability computations using a directed acyclic graph"@en ;
    skos:prefLabel "Bayesian Network"@en .

ai-owl:BayesianOptimisation a rdfs:Class,
        owl:Class,
        ai-owl:Technique ;
    dct:contributor _:Ne8d6151e3d8047e6a947b3ec1a3830a1 ;
    dct:created "2024-12-01"^^xsd:date ;
    rdfs:isDefinedBy ai-owl: ;
    rdfs:subClassOf ai-owl:StatisticalTechnique ;
    sw:term_status "accepted"@en ;
    skos:definition "Refers to Bayesian optimisation technique"@en ;
    skos:prefLabel "Bayesian Optimisation"@en .

ai-owl:BehaviourAnalysis a rdfs:Class,
        owl:Class,
        ai-owl:Capability ;
    dct:contributor _:Ne8d6151e3d8047e6a947b3ec1a3830a1 ;
    dct:created "2024-12-01"^^xsd:date ;
    rdfs:isDefinedBy ai-owl: ;
    rdfs:subClassOf ai-owl:HumanOrientedCapability ;
    sw:term_status "accepted"@en ;
    skos:definition "Capability of a system in analysing people's behaviour"@en ;
    skos:prefLabel "Behaviour Analysis"@en .

ai-owl:BiometricCapability a rdfs:Class,
        owl:Class,
        ai-owl:Capability ;
    dct:contributor _:Ne8d6151e3d8047e6a947b3ec1a3830a1 ;
    dct:created "2024-12-01"^^xsd:date ;
    rdfs:isDefinedBy ai-owl: ;
    rdfs:subClassOf ai-owl:HumanOrientedCapability ;
    sw:term_status "accepted"@en ;
    skos:definition "Capability involving processing of biometric data or related to biometrics"@en ;
    skos:prefLabel "Biometric Capability"@en .

ai-owl:BiometricCategorisation a rdfs:Class,
        owl:Class,
        ai-owl:Capability ;
    dct:contributor _:Ne8d6151e3d8047e6a947b3ec1a3830a1 ;
    dct:created "2024-12-01"^^xsd:date ;
    rdfs:isDefinedBy ai-owl: ;
    rdfs:subClassOf ai-owl:BiometricCapability ;
    sw:term_status "accepted"@en ;
    skos:definition "Capability involving assigning natural persons to specific categories based on their biometric data"@en ;
    skos:prefLabel "Biometric Categorisation"@en .

ai-owl:BiometricEmotionRecognition a rdfs:Class,
        owl:Class,
        ai-owl:Capability ;
    dct:contributor _:Ne8d6151e3d8047e6a947b3ec1a3830a1 ;
    dct:created "2024-12-01"^^xsd:date ;
    rdfs:isDefinedBy ai-owl: ;
    rdfs:subClassOf ai-owl:EmotionRecognition ;
    sw:term_status "accepted"@en ;
    skos:definition "Capability for recognisting emtions based on biometrics information"@en ;
    skos:prefLabel "Biometric Emotion Recognition"@en .

ai-owl:BiometricIdentification a rdfs:Class,
        owl:Class,
        ai-owl:Capability ;
    dct:contributor _:Ne8d6151e3d8047e6a947b3ec1a3830a1 ;
    dct:created "2024-12-01"^^xsd:date ;
    dct:source [ a schema:WebPage ;
            schema:name "The AI Act" ;
            schema:url "Recital 15 [https://eur-lex.europa.eu/legal-content/EN/TXT/HTML/?uri=OJ:L_202401689#rct_15]" ] ;
    rdfs:isDefinedBy ai-owl: ;
    rdfs:subClassOf ai-owl:BiometricCapability ;
    sw:term_status "accepted"@en ;
    skos:definition "Capability involving automated recognition of physical, physiological and behavioural human features such as the face, eye movement, body shape, voice, prosody, gait, posture, heart rate, blood pressure, odour, keystrokes characteristics, for the purpose of establishing an individual’s identity by comparing biometric data of that individual to stored biometric data of individuals in a reference database, irrespective of whether the individual has given its consent or not"@en ;
    skos:prefLabel "Biometric Identification"@en .

ai-owl:Capability a rdfs:Class,
        owl:Class ;
    dct:contributor _:Ne8d6151e3d8047e6a947b3ec1a3830a1 ;
    dct:created "2024-04-28"^^xsd:date ;
    rdfs:isDefinedBy ai-owl: ;
    rdfs:subClassOf ai-owl:AI ;
    sw:term_status "accepted"@en ;
    skos:definition "Capability or use of AI to achieve a technical goal or objective"@en ;
    skos:prefLabel "Capability"@en ;
    skos:scopeNote "This concept refers to the application of an AI technique to achieve a technical goal or function, and is necessary to distinguish the 'algorithm' (ai:Technique) from the 'application' (ai:Capability) and 'goal' (dpv:Purpose)"@en .

ai-owl:CognitiveComputing a rdfs:Class,
        owl:Class ;
    dct:contributor _:Ne8d6151e3d8047e6a947b3ec1a3830a1 ;
    dct:created "2024-12-01"^^xsd:date ;
    dct:source " 3.1.8"@en,
        "ISO/IEC 22989:2022"@en ;
    rdfs:isDefinedBy ai-owl: ;
    rdfs:subClassOf ai-owl:AISystem ;
    sw:term_status "accepted"@en ;
    skos:definition "Category of AI systems that enables people and machines to interact more naturally"@en ;
    skos:prefLabel "Cognitive Computing"@en .

ai-owl:ComputerVision a rdfs:Class,
        owl:Class,
        ai-owl:Capability ;
    dct:contributor _:Ne8d6151e3d8047e6a947b3ec1a3830a1 ;
    dct:created "2024-12-01"^^xsd:date ;
    dct:source " 3.7.1"@en,
        "ISO/IEC 22989:2022"@en ;
    rdfs:isDefinedBy ai-owl: ;
    rdfs:subClassOf ai-owl:Capability ;
    sw:term_status "accepted"@en ;
    skos:definition "Capability of a functional unit to acquire, process and interpret data representing images or video"@en ;
    skos:prefLabel "Computer Vision"@en .

ai-owl:ContentBasedRetrieval a rdfs:Class,
        owl:Class,
        ai-owl:Capability ;
    dct:contributor _:N0a43dd9ea5e94fe695d8b7df8802cfdd ;
    dct:created "2024-12-01"^^xsd:date ;
    rdfs:isDefinedBy ai-owl: ;
    rdfs:subClassOf ai-owl:InformationRetrieval ;
    sw:term_status "accepted"@en ;
    skos:definition "Capability for retrieval of information using the actual content to identify, select, filter, and provide results"@en ;
    skos:prefLabel "Content-based Retrieval"@en .

ai-owl:ContentGeneration a rdfs:Class,
        owl:Class,
        ai-owl:Capability ;
    dct:contributor _:N0a43dd9ea5e94fe695d8b7df8802cfdd,
        _:Ne8d6151e3d8047e6a947b3ec1a3830a1 ;
    dct:created "2024-12-01"^^xsd:date ;
    rdfs:isDefinedBy ai-owl: ;
    rdfs:subClassOf ai-owl:Capability ;
    sw:term_status "accepted"@en ;
    skos:definition "Capability to generate new content that is distinct from merely deriving or transforming existing content"@en ;
    skos:prefLabel "Content Generation"@en .

ai-owl:ContextAwareRetrieval a rdfs:Class,
        owl:Class,
        ai-owl:Capability ;
    dct:contributor _:N0a43dd9ea5e94fe695d8b7df8802cfdd ;
    dct:created "2024-12-01"^^xsd:date ;
    rdfs:isDefinedBy ai-owl: ;
    rdfs:subClassOf ai-owl:InformationRetrieval ;
    sw:term_status "accepted"@en ;
    skos:definition "Capability for retrieval of information that takes into account the user's context such as e.g., location, time, device, or activity to provide more relevant results"@en ;
    skos:prefLabel "Context-aware Retrieval"@en .

ai-owl:ContinuousValidationStage a rdfs:Class,
        owl:Class,
        ai-owl:LifecycleStage ;
    dct:contributor _:Ne8d6151e3d8047e6a947b3ec1a3830a1 ;
    dct:created "2024-12-01"^^xsd:date ;
    dct:source "ISO/IEC 22989:2032"@en ;
    rdfs:isDefinedBy ai-owl: ;
    rdfs:subClassOf ai-owl:LifecycleStage ;
    sw:term_status "accepted"@en ;
    skos:definition "The stage in the lifecycle where there is continuous learning within the AI system by incremental training on an ongoing basis while the system is running in production"@en ;
    skos:prefLabel "Continuous Validation Stage"@en .

ai-owl:ConvolutionalNeuralNetwork a rdfs:Class,
        owl:Class,
        ai-owl:Technique ;
    dct:contributor _:Ne8d6151e3d8047e6a947b3ec1a3830a1 ;
    dct:created "2024-12-01"^^xsd:date ;
    dct:source " 3.4.2"@en,
        "ISO/IEC 22989"@en ;
    rdfs:isDefinedBy ai-owl: ;
    rdfs:subClassOf ai-owl:NeuralNetwork ;
    sw:term_status "accepted"@en ;
    skos:definition "Feed forward neural network using convolution  in at least one of its layers"@en ;
    skos:prefLabel "Convolutional Neural Network (CNN)"@en .

ai-owl:Data a rdfs:Class,
        owl:Class ;
    dct:contributor _:Ne8d6151e3d8047e6a947b3ec1a3830a1 ;
    dct:created "2024-12-01"^^xsd:date ;
    rdfs:isDefinedBy ai-owl: ;
    rdfs:subClassOf dpv-owl:Data,
        tech-owl:InputOutput ;
    sw:term_status "accepted"@en ;
    skos:definition "Data involved in the development and use of an AI system or model"@en ;
    skos:prefLabel "AI Data"@en .

ai-owl:DataAggregationBias a rdfs:Class,
        owl:Class,
        dpv-owl:RiskConcept,
        risk-owl:PotentialRisk,
        risk-owl:PotentialRiskSource ;
    dct:contributor _:N606ea170c32e4fb5ac26e62242d8681b,
        _:Ne8d6151e3d8047e6a947b3ec1a3830a1 ;
    dct:created "2024-09-13"^^xsd:date ;
    dct:source "ISO/IEC 24027:2021"@en ;
    rdfs:isDefinedBy ai-owl: ;
    rdfs:subClassOf ai-owl:DataBias ;
    sw:term_status "accepted"@en ;
    skos:definition "Bias that occurs from aggregating data covering different groups of objects that might have different statistical distributions which introduce bias into the data used to train AI systems"@en ;
    skos:prefLabel "Data Aggregation Bias"@en .

ai-owl:DataBias a rdfs:Class,
        owl:Class,
        dpv-owl:RiskConcept,
        risk-owl:PotentialRisk,
        risk-owl:PotentialRiskSource ;
    dct:contributor _:N606ea170c32e4fb5ac26e62242d8681b,
        _:Ne8d6151e3d8047e6a947b3ec1a3830a1 ;
    dct:created "2024-09-13"^^xsd:date ;
    dct:source "ISO/IEC 24027:2021"@en ;
    rdfs:isDefinedBy ai-owl: ;
    rdfs:subClassOf ai-owl:AIBias ;
    sw:term_status "accepted"@en ;
    skos:definition "Bias that occurs due to unaddressed data properties that lead to AI systems that perform better or worse for different groups"@en ;
    skos:prefLabel "Data Bias"@en .

ai-owl:DataLabelsAndLabellingProcessBias a rdfs:Class,
        owl:Class,
        dpv-owl:RiskConcept,
        risk-owl:PotentialRisk,
        risk-owl:PotentialRiskSource ;
    dct:contributor _:N606ea170c32e4fb5ac26e62242d8681b,
        _:Ne8d6151e3d8047e6a947b3ec1a3830a1 ;
    dct:created "2024-09-13"^^xsd:date ;
    dct:source "ISO/IEC 24027:2021"@en ;
    rdfs:isDefinedBy ai-owl: ;
    rdfs:subClassOf ai-owl:DataBias ;
    sw:term_status "accepted"@en ;
    skos:definition "Bias that occurs due to the labelling process itself introducing societal or cognitive biases"@en ;
    skos:prefLabel "Data Labels And Labelling Process Bias"@en .

ai-owl:DataPoisoning a rdfs:Class,
        owl:Class,
        dpv-owl:RiskConcept,
        risk-owl:IntegrityConcept,
        risk-owl:PotentialConsequence,
        risk-owl:PotentialRisk,
        risk-owl:PotentialRiskSource ;
    dct:contributor _:Ne8d6151e3d8047e6a947b3ec1a3830a1 ;
    dct:created "2024-12-01"^^xsd:date ;
    rdfs:isDefinedBy ai-owl: ;
    rdfs:subClassOf ai-owl:SecurityAttack ;
    sw:term_status "accepted"@en ;
    skos:definition "Attack trying to manipulate the training dataset"@en ;
    skos:prefLabel "Data Poisoning"@en .

ai-owl:DataRisk a rdfs:Class,
        owl:Class,
        dpv-owl:RiskConcept,
        risk-owl:PotentialRisk,
        risk-owl:PotentialRiskSource ;
    dct:contributor _:Ne8d6151e3d8047e6a947b3ec1a3830a1 ;
    dct:created "2024-12-01"^^xsd:date ;
    rdfs:isDefinedBy ai-owl: ;
    rdfs:subClassOf ai-owl:RiskConcept ;
    sw:term_status "accepted"@en ;
    skos:definition "Risk associated with data used or produced or otherwise involved in the context of AI"@en ;
    skos:prefLabel "Data Risk"@en .

ai-owl:DecisionTree a rdfs:Class,
        owl:Class,
        ai-owl:Technique ;
    dct:contributor _:Ne8d6151e3d8047e6a947b3ec1a3830a1 ;
    dct:created "2024-12-01"^^xsd:date ;
    dct:source " 3.3.2"@en,
        "ISO/IEC 22989"@en ;
    rdfs:isDefinedBy ai-owl: ;
    rdfs:subClassOf ai-owl:StatisticalTechnique ;
    sw:term_status "accepted"@en ;
    skos:definition "Technique for which inference is encoded as paths from the root to a leaf node in a tree structure"@en ;
    skos:prefLabel "Decision Tree"@en .

ai-owl:DecomissionStage a rdfs:Class,
        owl:Class,
        ai-owl:LifecycleStage ;
    dct:contributor _:N0a43dd9ea5e94fe695d8b7df8802cfdd ;
    dct:created "2024-12-01"^^xsd:date ;
    dct:source "ISO/IEC 22989:2035"@en ;
    rdfs:isDefinedBy ai-owl: ;
    rdfs:subClassOf ai-owl:RetirementStage ;
    sw:term_status "accepted"@en ;
    skos:definition "The stage in the lifecycle where the AI system is being decomissioned as part of retirement"@en ;
    skos:prefLabel "Decommission Stage"@en .

ai-owl:DeepLearning a rdfs:Class,
        owl:Class,
        ai-owl:Technique ;
    dct:contributor _:Ne8d6151e3d8047e6a947b3ec1a3830a1 ;
    dct:created "2024-12-01"^^xsd:date ;
    dct:source " 3.4.4"@en,
        "ISO/IEC 22989:2022"@en ;
    rdfs:isDefinedBy ai-owl: ;
    rdfs:subClassOf ai-owl:MachineLearning ;
    sw:term_status "accepted"@en ;
    skos:definition "Approach to creating rich hierarchical representations through the training of neural networks with many hidden layers"@en ;
    skos:prefLabel "Deep Learning"@en .

ai-owl:DeploymentStage a rdfs:Class,
        owl:Class,
        ai-owl:LifecycleStage ;
    dct:contributor _:Ne8d6151e3d8047e6a947b3ec1a3830a1 ;
    dct:created "2024-12-01"^^xsd:date ;
    dct:source "ISO/IEC 22989:2027"@en ;
    rdfs:isDefinedBy ai-owl: ;
    rdfs:subClassOf ai-owl:LifecycleStage ;
    sw:term_status "accepted"@en ;
    skos:definition "The stage in the lifecycle where  the AI system is installed, released or configured for deployment and operation in a target environment"@en ;
    skos:prefLabel "Deployment Stage"@en .

ai-owl:DesignStage a rdfs:Class,
        owl:Class,
        ai-owl:LifecycleStage ;
    dct:contributor _:Ne8d6151e3d8047e6a947b3ec1a3830a1 ;
    dct:created "2024-12-01"^^xsd:date ;
    dct:source "ISO/IEC 22989:2023"@en ;
    rdfs:isDefinedBy ai-owl: ;
    rdfs:subClassOf ai-owl:LifecycleStage ;
    sw:term_status "accepted"@en ;
    skos:definition "The stage in the lifecycle where designs are created for the AI system"@en ;
    skos:prefLabel "Design Stage"@en .

ai-owl:DevelopmentStage a rdfs:Class,
        owl:Class,
        ai-owl:LifecycleStage ;
    dct:contributor _:Ne8d6151e3d8047e6a947b3ec1a3830a1 ;
    dct:created "2024-12-01"^^xsd:date ;
    dct:source "ISO/IEC 22989:2024"@en ;
    rdfs:isDefinedBy ai-owl: ;
    rdfs:subClassOf ai-owl:LifecycleStage ;
    sw:term_status "accepted"@en ;
    skos:definition "The stage in the lifecycle where the development and creation of the system occurs, signalling upon completion that it is ready for verification and validation"@en ;
    skos:prefLabel "Development Stage"@en .

ai-owl:DialogueManagement a rdfs:Class,
        owl:Class,
        ai-owl:Capability ;
    dct:contributor _:Ne8d6151e3d8047e6a947b3ec1a3830a1 ;
    dct:created "2024-12-01"^^xsd:date ;
    dct:source " 3.6.2"@en,
        "ISO/IEC 22989:2022"@en ;
    rdfs:isDefinedBy ai-owl: ;
    rdfs:subClassOf ai-owl:LanguageCapability ;
    sw:term_status "accepted"@en ;
    skos:definition "Capability for choosing the appropriate next move in a dialogue based on user input, the dialogue history and other contextual knowledge to meet a desired goal"@en ;
    skos:prefLabel "Dialogue Management"@en .

ai-owl:DiscardStage a rdfs:Class,
        owl:Class,
        ai-owl:LifecycleStage ;
    dct:contributor _:N0a43dd9ea5e94fe695d8b7df8802cfdd ;
    dct:created "2024-12-01"^^xsd:date ;
    dct:source "ISO/IEC 22989:2036"@en ;
    rdfs:isDefinedBy ai-owl: ;
    rdfs:subClassOf ai-owl:RetirementStage ;
    sw:term_status "accepted"@en ;
    skos:definition "The stage in the lifecycle where the AI system is being discarded as part of retirement"@en ;
    skos:prefLabel "Discard Stage"@en .

ai-owl:DistributedTrainingBias a rdfs:Class,
        owl:Class,
        dpv-owl:RiskConcept,
        risk-owl:PotentialRisk,
        risk-owl:PotentialRiskSource ;
    dct:contributor _:N606ea170c32e4fb5ac26e62242d8681b,
        _:Ne8d6151e3d8047e6a947b3ec1a3830a1 ;
    dct:created "2024-09-13"^^xsd:date ;
    dct:source "ISO/IEC 24027:2021"@en ;
    rdfs:isDefinedBy ai-owl: ;
    rdfs:subClassOf ai-owl:DataBias ;
    sw:term_status "accepted"@en ;
    skos:definition "Bias that occurs due to distributed machine having different sources of data that do not have the same distribution of feature space"@en ;
    skos:prefLabel "Distributed Training Bias"@en .

ai-owl:EmotionRecognition a rdfs:Class,
        owl:Class,
        ai-owl:Capability ;
    dct:contributor _:Ne8d6151e3d8047e6a947b3ec1a3830a1 ;
    dct:created "2024-12-01"^^xsd:date ;
    dct:source " 3.6.3"@en,
        "ISO/IEC 22989:2022"@en ;
    rdfs:isDefinedBy ai-owl: ;
    rdfs:subClassOf ai-owl:HumanOrientedCapability ;
    sw:term_status "accepted"@en ;
    skos:definition "Capability for identifying and categorizing emotions expressed in a piece of text, speech, video or image or combination thereof"@en ;
    skos:prefLabel "Emotion Recognition"@en .

ai-owl:EngineeringDecisionBias a rdfs:Class,
        owl:Class,
        dpv-owl:RiskConcept,
        risk-owl:PotentialRisk,
        risk-owl:PotentialRiskSource ;
    dct:contributor _:N606ea170c32e4fb5ac26e62242d8681b,
        _:Ne8d6151e3d8047e6a947b3ec1a3830a1 ;
    dct:created "2024-09-13"^^xsd:date ;
    dct:source "ISO/IEC 24027:2021"@en ;
    rdfs:isDefinedBy ai-owl: ;
    rdfs:subClassOf ai-owl:AIBias ;
    sw:term_status "accepted"@en ;
    skos:definition "Bias that occurs due to machine learning model architectures - encompassing all model specifications, parameters and manually designed features"@en ;
    skos:prefLabel "Engineering Decision Bias"@en ;
    skos:scopeNote "Data bias and human cognitive bias can contribute to such bias"@en .

ai-owl:ExpertSystem a rdfs:Class,
        owl:Class ;
    dct:contributor _:Ne8d6151e3d8047e6a947b3ec1a3830a1 ;
    dct:created "2024-12-01"^^xsd:date ;
    dct:source " 3.1.13"@en,
        "ISO/IEC 22989:2022"@en ;
    rdfs:isDefinedBy ai-owl: ;
    rdfs:subClassOf ai-owl:AISystem ;
    sw:term_status "accepted"@en ;
    skos:definition "AI system that accumulates, combines and encapsulates knowledge provided by a human expert or experts in a specific domain to infer solutions to problems"@en ;
    skos:prefLabel "Expert System"@en .

ai-owl:FaceRecognition a rdfs:Class,
        owl:Class,
        ai-owl:Capability ;
    dct:contributor _:Ne8d6151e3d8047e6a947b3ec1a3830a1 ;
    dct:created "2024-12-01"^^xsd:date ;
    dct:source " 3.7.2"@en,
        "ISO/IEC 22989:2022"@en ;
    rdfs:isDefinedBy ai-owl: ;
    rdfs:subClassOf ai-owl:BiometricCapability,
        ai-owl:ComputerVision ;
    sw:term_status "accepted"@en ;
    skos:definition "Capability involving automatic pattern recognition for comparing stored images of human faces with the image of an actual face, indicating any matching, if it exists, and any data, if they exist, identifying the person to whom the face belongs"@en ;
    skos:prefLabel "Face Recognition"@en .

ai-owl:FeatureEngineeringBias a rdfs:Class,
        owl:Class,
        dpv-owl:RiskConcept,
        risk-owl:PotentialRisk,
        risk-owl:PotentialRiskSource ;
    dct:contributor _:N606ea170c32e4fb5ac26e62242d8681b,
        _:Ne8d6151e3d8047e6a947b3ec1a3830a1 ;
    dct:created "2024-09-13"^^xsd:date ;
    dct:source "ISO/IEC 24027:2021"@en ;
    rdfs:isDefinedBy ai-owl: ;
    rdfs:subClassOf ai-owl:EngineeringDecisionBias ;
    sw:term_status "accepted"@en ;
    skos:definition "Bias that occurs from steps such as encoding, data type conversion, dimensionality reduction and feature selection which are subject to choices made by the AI developer and introduce bias in the ML model"@en ;
    skos:prefLabel "Feature Engineering Bias"@en .

ai-owl:FeedForwardNeuralNetwork a rdfs:Class,
        owl:Class,
        ai-owl:Technique ;
    dct:contributor _:Ne8d6151e3d8047e6a947b3ec1a3830a1 ;
    dct:created "2024-12-01"^^xsd:date ;
    dct:source " 3.4.6"@en,
        "ISO/IEC 22989"@en ;
    rdfs:isDefinedBy ai-owl: ;
    rdfs:subClassOf ai-owl:NeuralNetwork ;
    sw:term_status "accepted"@en ;
    skos:definition "Neural network where information is fed from the input layer to the output layer in one direction only"@en ;
    skos:prefLabel "Feed Forward Neural Network"@en .

ai-owl:GPAIModel a rdfs:Class,
        owl:Class ;
    dct:contributor _:Ne8d6151e3d8047e6a947b3ec1a3830a1 ;
    dct:created "2024-12-01"^^xsd:date ;
    dct:source "EU AI Act"@en ;
    rdfs:isDefinedBy ai-owl: ;
    rdfs:subClassOf ai-owl:Model ;
    sw:term_status "accepted"@en ;
    skos:definition "A model that displays generality in terms of capabilities and potential applications"@en ;
    skos:prefLabel "General Purpose AI Model"@en .

ai-owl:GeneticAlgorithm a rdfs:Class,
        owl:Class,
        ai-owl:Technique ;
    dct:contributor _:Ne8d6151e3d8047e6a947b3ec1a3830a1 ;
    dct:created "2024-12-01"^^xsd:date ;
    dct:source " 3.1.15"@en,
        "ISO/IEC 22989:2022"@en ;
    rdfs:isDefinedBy ai-owl: ;
    rdfs:subClassOf ai-owl:Technique ;
    sw:term_status "accepted"@en ;
    skos:definition "Algorithm which simulates natural selection by creating and evolving a population of individuals (solutions) for optimization problems"@en ;
    skos:prefLabel "Genetic Algorithm"@en .

ai-owl:GestureRecognition a rdfs:Class,
        owl:Class,
        ai-owl:Capability ;
    dct:contributor _:Ne8d6151e3d8047e6a947b3ec1a3830a1 ;
    dct:created "2024-12-01"^^xsd:date ;
    dct:source " Defining Artificial Intelligence 2.0"@en,
        "AI Watch"@en ;
    rdfs:isDefinedBy ai-owl: ;
    rdfs:subClassOf ai-owl:BiometricCapability,
        ai-owl:ComputerVision ;
    sw:term_status "accepted"@en ;
    skos:definition "Capability for recognising human gestures"@en ;
    skos:prefLabel "Gesture Recognition"@en .

ai-owl:HumanOrientedCapability a rdfs:Class,
        owl:Class,
        ai-owl:Capability ;
    dct:contributor _:N0a43dd9ea5e94fe695d8b7df8802cfdd ;
    dct:created "2024-12-01"^^xsd:date ;
    rdfs:isDefinedBy ai-owl: ;
    rdfs:subClassOf ai-owl:Capability ;
    sw:term_status "accepted"@en ;
    skos:definition "Capabilities that are inherently about humans or oriented towards human characteristics and activities"@en ;
    skos:prefLabel "Human-Oriented Capability"@en .

ai-owl:HyperparameterTuningBias a rdfs:Class,
        owl:Class,
        dpv-owl:RiskConcept,
        risk-owl:PotentialRisk,
        risk-owl:PotentialRiskSource ;
    dct:contributor _:N606ea170c32e4fb5ac26e62242d8681b,
        _:Ne8d6151e3d8047e6a947b3ec1a3830a1 ;
    dct:created "2024-09-13"^^xsd:date ;
    dct:source "ISO/IEC 24027:2021"@en ;
    rdfs:isDefinedBy ai-owl: ;
    rdfs:subClassOf ai-owl:EngineeringDecisionBias ;
    sw:term_status "accepted"@en ;
    skos:definition "Bias that occurs from hyperparameters defining how the model is structured and which cannot be directly trained from the data like model parameters, where hyperparameters affect the model functioning and accuracy of the model"@en ;
    skos:prefLabel "Hyperparameter Tuning Bias"@en .

ai-owl:ImageGeneration a rdfs:Class,
        owl:Class,
        ai-owl:Capability ;
    dct:contributor _:N0a43dd9ea5e94fe695d8b7df8802cfdd,
        _:Ne8d6151e3d8047e6a947b3ec1a3830a1 ;
    dct:created "2024-12-01"^^xsd:date ;
    rdfs:isDefinedBy ai-owl: ;
    rdfs:subClassOf ai-owl:ContentGeneration ;
    sw:term_status "accepted"@en ;
    skos:definition "Capability to generate image"@en ;
    skos:prefLabel "Image Generation"@en .

ai-owl:ImageRecognition a rdfs:Class,
        owl:Class,
        ai-owl:Capability ;
    dct:contributor _:Ne8d6151e3d8047e6a947b3ec1a3830a1 ;
    dct:created "2024-12-01"^^xsd:date ;
    dct:source " 3.7.4"@en,
        "ISO/IEC 22989:2022"@en ;
    rdfs:isDefinedBy ai-owl: ;
    rdfs:subClassOf ai-owl:ComputerVision ;
    sw:term_status "accepted"@en ;
    skos:definition "Capability for image classification process that classifies object(s), pattern(s) or concept(s) in an image"@en ;
    skos:prefLabel "Image Recognition"@en .

ai-owl:InceptionStage a rdfs:Class,
        owl:Class,
        ai-owl:LifecycleStage ;
    dct:contributor _:Ne8d6151e3d8047e6a947b3ec1a3830a1 ;
    dct:created "2024-12-01"^^xsd:date ;
    dct:source "ISO/IEC 22989:2022"@en ;
    rdfs:isDefinedBy ai-owl: ;
    rdfs:subClassOf ai-owl:LifecycleStage ;
    sw:term_status "accepted"@en ;
    skos:definition "The stage in the lifecycle where inception regarding AI occurs and one or more stakeholders decide to turn an idea into a tangible system"@en ;
    skos:prefLabel "Inception Stage"@en .

ai-owl:IncidentMonitoringStage a rdfs:Class,
        owl:Class,
        ai-owl:LifecycleStage ;
    dct:contributor _:N0a43dd9ea5e94fe695d8b7df8802cfdd ;
    dct:created "2024-12-01"^^xsd:date ;
    dct:source "ISO/IEC 22989:2029"@en ;
    rdfs:isDefinedBy ai-owl: ;
    rdfs:subClassOf ai-owl:OperationStage ;
    sw:term_status "accepted"@en ;
    skos:definition "The stage in the lifecycle where an AI system is actively being monitored for incidents"@en ;
    skos:prefLabel "Incident Monitoring Stage"@en .

ai-owl:InductiveProgramming a rdfs:Class,
        owl:Class,
        ai-owl:Technique ;
    dct:contributor _:Ne8d6151e3d8047e6a947b3ec1a3830a1 ;
    dct:created "2024-12-01"^^xsd:date ;
    rdfs:isDefinedBy ai-owl: ;
    rdfs:subClassOf ai-owl:KnowledgeTechnique ;
    sw:term_status "accepted"@en ;
    skos:definition "An algorithm or program featuring recursive calls or repetition control structures"@en ;
    skos:prefLabel "Inductive Programming"@en .

ai-owl:IndustrialRobot a rdfs:Class,
        owl:Class ;
    dct:contributor _:Ne8d6151e3d8047e6a947b3ec1a3830a1 ;
    dct:created "2024-12-01"^^xsd:date ;
    dct:source " 3.1.29"@en,
        "ISO/IEC 22989:2022"@en ;
    rdfs:isDefinedBy ai-owl: ;
    rdfs:subClassOf ai-owl:Robot ;
    sw:term_status "accepted"@en ;
    skos:definition "A robot or robotic system for use in industrial automation applications"@en ;
    skos:prefLabel "Industrial Robot"@en .

ai-owl:InformationRetrieval a rdfs:Class,
        owl:Class,
        ai-owl:Capability ;
    dct:contributor _:Ne8d6151e3d8047e6a947b3ec1a3830a1 ;
    dct:created "2024-12-01"^^xsd:date ;
    dct:source " 3.6.4"@en,
        "ISO/IEC 22989:2022"@en ;
    rdfs:isDefinedBy ai-owl: ;
    rdfs:subClassOf ai-owl:Capability ;
    sw:term_status "accepted"@en ;
    skos:definition "Capability for retrieving relevant documents or parts of documents from a dataset, typically based on keyword or natural language queries"@en ;
    skos:prefLabel "Information Retrieval (IR)"@en .

ai-owl:InformativenessBias a rdfs:Class,
        owl:Class,
        dpv-owl:RiskConcept,
        risk-owl:PotentialRisk,
        risk-owl:PotentialRiskSource ;
    dct:contributor _:N606ea170c32e4fb5ac26e62242d8681b,
        _:Ne8d6151e3d8047e6a947b3ec1a3830a1 ;
    dct:created "2024-09-13"^^xsd:date ;
    dct:source "ISO/IEC 24027:2021"@en ;
    rdfs:isDefinedBy ai-owl: ;
    rdfs:subClassOf ai-owl:EngineeringDecisionBias ;
    sw:term_status "accepted"@en ;
    skos:definition "Bias that occurs or some groups, the mapping between inputs present in the data and outputs are more difficult to learn and where a model that only has one feature set available, can be biased against the group whose relationships are difficult to learn from available data"@en ;
    skos:prefLabel "Informativeness Bias"@en ;
    skos:scopeNote "This can happen when some features are highly informative about one group, while a different set of features is highly informative about another group. If this is the case, then a model that only has one feature set available, can be biased against the group whose relationships are difficult to learn from available data"@en .

ai-owl:InputDataBias a rdfs:Class,
        owl:Class,
        dpv-owl:RiskConcept,
        risk-owl:PotentialRisk,
        risk-owl:PotentialRiskSource ;
    dct:contributor _:Ne8d6151e3d8047e6a947b3ec1a3830a1 ;
    dct:created "2024-12-01"^^xsd:date ;
    rdfs:isDefinedBy ai-owl: ;
    rdfs:subClassOf ai-owl:InputDataRisk ;
    sw:term_status "accepted"@en ;
    skos:definition "Concept representing input data containing or potentially containing bias"@en ;
    skos:prefLabel "Input Data Bias"@en .

ai-owl:InputDataInaccurate a rdfs:Class,
        owl:Class,
        dpv-owl:RiskConcept,
        risk-owl:PotentialRisk,
        risk-owl:PotentialRiskSource ;
    dct:contributor _:Ne8d6151e3d8047e6a947b3ec1a3830a1 ;
    dct:created "2024-12-01"^^xsd:date ;
    rdfs:isDefinedBy ai-owl: ;
    rdfs:subClassOf ai-owl:InputDataRisk ;
    sw:term_status "accepted"@en ;
    skos:definition "Concept representing input data being inaccurate"@en ;
    skos:prefLabel "Input Data Inaccurate"@en .

ai-owl:InputDataInappropriate a rdfs:Class,
        owl:Class,
        dpv-owl:RiskConcept,
        risk-owl:PotentialRisk,
        risk-owl:PotentialRiskSource ;
    dct:contributor _:Ne8d6151e3d8047e6a947b3ec1a3830a1 ;
    dct:created "2024-12-01"^^xsd:date ;
    rdfs:isDefinedBy ai-owl: ;
    rdfs:subClassOf ai-owl:InputDataRisk ;
    sw:term_status "accepted"@en ;
    skos:definition "Concept representing input data being inappropriate"@en ;
    skos:prefLabel "Input Data Inappropriate"@en .

ai-owl:InputDataIncomplete a rdfs:Class,
        owl:Class,
        dpv-owl:RiskConcept,
        risk-owl:PotentialRisk,
        risk-owl:PotentialRiskSource ;
    dct:contributor _:Ne8d6151e3d8047e6a947b3ec1a3830a1 ;
    dct:created "2024-12-01"^^xsd:date ;
    rdfs:isDefinedBy ai-owl: ;
    rdfs:subClassOf ai-owl:InputDataRisk ;
    sw:term_status "accepted"@en ;
    skos:definition "Concept representing input data being incomplete"@en ;
    skos:prefLabel "Input Data Incomplete"@en .

ai-owl:InputDataInconsistent a rdfs:Class,
        owl:Class,
        dpv-owl:RiskConcept,
        risk-owl:PotentialRisk,
        risk-owl:PotentialRiskSource ;
    dct:contributor _:Ne8d6151e3d8047e6a947b3ec1a3830a1 ;
    dct:created "2024-12-01"^^xsd:date ;
    rdfs:isDefinedBy ai-owl: ;
    rdfs:subClassOf ai-owl:InputDataRisk ;
    sw:term_status "accepted"@en ;
    skos:definition "Concept representing input data being inconsistent"@en ;
    skos:prefLabel "Input Data Inconsistent"@en .

ai-owl:InputDataMisclassified a rdfs:Class,
        owl:Class,
        dpv-owl:RiskConcept,
        risk-owl:PotentialRisk,
        risk-owl:PotentialRiskSource ;
    dct:contributor _:Ne8d6151e3d8047e6a947b3ec1a3830a1 ;
    dct:created "2024-12-01"^^xsd:date ;
    rdfs:isDefinedBy ai-owl: ;
    rdfs:subClassOf ai-owl:InputDataRisk ;
    sw:term_status "accepted"@en ;
    skos:definition "Concept representing input data being misclassified"@en ;
    skos:prefLabel "Input Data Misclassified"@en .

ai-owl:InputDataMisinterpretation a rdfs:Class,
        owl:Class,
        dpv-owl:RiskConcept,
        risk-owl:PotentialRisk,
        risk-owl:PotentialRiskSource ;
    dct:contributor _:Ne8d6151e3d8047e6a947b3ec1a3830a1 ;
    dct:created "2024-12-01"^^xsd:date ;
    rdfs:isDefinedBy ai-owl: ;
    rdfs:subClassOf ai-owl:InputDataRisk ;
    sw:term_status "accepted"@en ;
    skos:definition "Concept representing input data being misinterpretation"@en ;
    skos:prefLabel "Input Data Misinterpretation"@en .

ai-owl:InputDataNoise a rdfs:Class,
        owl:Class,
        dpv-owl:RiskConcept,
        risk-owl:PotentialRisk,
        risk-owl:PotentialRiskSource ;
    dct:contributor _:Ne8d6151e3d8047e6a947b3ec1a3830a1 ;
    dct:created "2024-12-01"^^xsd:date ;
    rdfs:isDefinedBy ai-owl: ;
    rdfs:subClassOf ai-owl:InputDataRisk ;
    sw:term_status "accepted"@en ;
    skos:definition "Concept representing input data being noise"@en ;
    skos:prefLabel "Input Data Noise"@en .

ai-owl:InputDataOutdated a rdfs:Class,
        owl:Class,
        dpv-owl:RiskConcept,
        risk-owl:PotentialRisk,
        risk-owl:PotentialRiskSource ;
    dct:contributor _:Ne8d6151e3d8047e6a947b3ec1a3830a1 ;
    dct:created "2024-12-01"^^xsd:date ;
    rdfs:isDefinedBy ai-owl: ;
    rdfs:subClassOf ai-owl:InputDataRisk ;
    sw:term_status "accepted"@en ;
    skos:definition "Concept representing input data being outdated"@en ;
    skos:prefLabel "Input Data Outdated"@en .

ai-owl:InputDataRisk a rdfs:Class,
        owl:Class,
        dpv-owl:RiskConcept,
        risk-owl:PotentialRisk,
        risk-owl:PotentialRiskSource ;
    dct:contributor _:Ne8d6151e3d8047e6a947b3ec1a3830a1 ;
    dct:created "2024-12-01"^^xsd:date ;
    rdfs:isDefinedBy ai-owl: ;
    rdfs:subClassOf ai-owl:DataRisk ;
    sw:term_status "accepted"@en ;
    skos:definition "Risks and risk concepts related to input data"@en ;
    skos:prefLabel "Input Data Risk"@en .

ai-owl:InputDataSelectionError a rdfs:Class,
        owl:Class,
        dpv-owl:RiskConcept,
        risk-owl:PotentialRisk,
        risk-owl:PotentialRiskSource ;
    dct:contributor _:Ne8d6151e3d8047e6a947b3ec1a3830a1 ;
    dct:created "2024-12-01"^^xsd:date ;
    rdfs:isDefinedBy ai-owl: ;
    rdfs:subClassOf ai-owl:InputDataRisk ;
    sw:term_status "accepted"@en ;
    skos:definition "Concept representing an error in input data selection"@en ;
    skos:prefLabel "Input Data Selection Error"@en .

ai-owl:InputDataSparse a rdfs:Class,
        owl:Class,
        dpv-owl:RiskConcept,
        risk-owl:PotentialRisk,
        risk-owl:PotentialRiskSource ;
    dct:contributor _:Ne8d6151e3d8047e6a947b3ec1a3830a1 ;
    dct:created "2024-12-01"^^xsd:date ;
    rdfs:isDefinedBy ai-owl: ;
    rdfs:subClassOf ai-owl:InputDataRisk ;
    sw:term_status "accepted"@en ;
    skos:definition "Concept representing input data being sparse"@en ;
    skos:prefLabel "Input Data Sparse"@en .

ai-owl:InputDataUnrepresentative a rdfs:Class,
        owl:Class,
        dpv-owl:RiskConcept,
        risk-owl:PotentialRisk,
        risk-owl:PotentialRiskSource ;
    dct:contributor _:Ne8d6151e3d8047e6a947b3ec1a3830a1 ;
    dct:created "2024-12-01"^^xsd:date ;
    rdfs:isDefinedBy ai-owl: ;
    rdfs:subClassOf ai-owl:InputDataRisk ;
    sw:term_status "accepted"@en ;
    skos:definition "Concept representing input data being unrepresentative"@en ;
    skos:prefLabel "Input Data Unrepresentative"@en .

ai-owl:InputDataUnstructured a rdfs:Class,
        owl:Class,
        dpv-owl:RiskConcept,
        risk-owl:PotentialRisk,
        risk-owl:PotentialRiskSource ;
    dct:contributor _:Ne8d6151e3d8047e6a947b3ec1a3830a1 ;
    dct:created "2024-12-01"^^xsd:date ;
    rdfs:isDefinedBy ai-owl: ;
    rdfs:subClassOf ai-owl:InputDataRisk ;
    sw:term_status "accepted"@en ;
    skos:definition "Concept representing input data being unstructured"@en ;
    skos:prefLabel "Input Data Unstructured"@en .

ai-owl:InputDataUnverified a rdfs:Class,
        owl:Class,
        dpv-owl:RiskConcept,
        risk-owl:PotentialRisk,
        risk-owl:PotentialRiskSource ;
    dct:contributor _:Ne8d6151e3d8047e6a947b3ec1a3830a1 ;
    dct:created "2024-12-01"^^xsd:date ;
    rdfs:isDefinedBy ai-owl: ;
    rdfs:subClassOf ai-owl:InputDataRisk ;
    sw:term_status "accepted"@en ;
    skos:definition "Concept representing input data being unverified"@en ;
    skos:prefLabel "Input Data Unverified"@en .

ai-owl:IntelligentControlSystem a rdfs:Class,
        owl:Class ;
    dct:contributor _:Ne8d6151e3d8047e6a947b3ec1a3830a1 ;
    dct:created "2024-12-01"^^xsd:date ;
    dct:source " Defining Artificial Intelligence 2.0"@en,
        "AI Watch"@en ;
    rdfs:isDefinedBy ai-owl: ;
    rdfs:subClassOf ai-owl:AISystem ;
    sw:term_status "accepted"@en ;
    skos:definition "Category of AI systems which implement intelligent control principles for real-world applications by using AI capabilities and techniques"@en ;
    skos:prefLabel "Intelligent Control System"@en .

ai-owl:KnowledgeRepresentation a rdfs:Class,
        owl:Class,
        ai-owl:Technique ;
    dct:contributor _:Ne8d6151e3d8047e6a947b3ec1a3830a1 ;
    dct:created "2024-12-01"^^xsd:date ;
    rdfs:isDefinedBy ai-owl: ;
    rdfs:subClassOf ai-owl:KnowledgeTechnique ;
    sw:term_status "accepted"@en ;
    skos:definition "Encoding knowledge in a formal language"@en ;
    skos:prefLabel "Knowledge Representation"@en .

ai-owl:KnowledgeTechnique a rdfs:Class,
        owl:Class,
        ai-owl:Technique ;
    dct:contributor _:Ne8d6151e3d8047e6a947b3ec1a3830a1 ;
    dct:created "2024-12-01"^^xsd:date ;
    rdfs:isDefinedBy ai-owl: ;
    rdfs:subClassOf ai-owl:Technique ;
    sw:term_status "accepted"@en ;
    skos:definition "Techniques based on the use of knowledge bases"@en ;
    skos:prefLabel "Knowledge Technique"@en .

ai-owl:LanguageCapability a rdfs:Class,
        owl:Class,
        ai-owl:Capability ;
    dct:contributor _:N0a43dd9ea5e94fe695d8b7df8802cfdd ;
    dct:created "2024-12-01"^^xsd:date ;
    rdfs:isDefinedBy ai-owl: ;
    rdfs:subClassOf ai-owl:Capability ;
    sw:term_status "accepted"@en ;
    skos:definition "Capabilities related to languages"@en ;
    skos:prefLabel "Language Capability"@en .

ai-owl:LieDetection a rdfs:Class,
        owl:Class,
        ai-owl:Capability ;
    dct:contributor _:Ne8d6151e3d8047e6a947b3ec1a3830a1 ;
    dct:created "2024-12-01"^^xsd:date ;
    rdfs:isDefinedBy ai-owl: ;
    rdfs:subClassOf ai-owl:HumanOrientedCapability ;
    sw:term_status "accepted"@en ;
    skos:definition "Capability to detect lies in the context of human speech, behaviour, information, or activities"@en ;
    skos:prefLabel "Lie Detection"@en .

ai-owl:LifecycleStage a rdfs:Class,
        owl:Class ;
    dct:contributor _:Ne8d6151e3d8047e6a947b3ec1a3830a1 ;
    dct:created "2024-12-01"^^xsd:date ;
    rdfs:isDefinedBy ai-owl: ;
    rdfs:subClassOf tech-owl:LifecycleStage ;
    sw:term_status "accepted"@en ;
    skos:definition "A stage in the lifecycle of AI"@en ;
    skos:prefLabel "Lifecycle Stage"@en .

ai-owl:LocalBiometricIdentification a rdfs:Class,
        owl:Class,
        ai-owl:Capability ;
    dct:contributor _:N0a43dd9ea5e94fe695d8b7df8802cfdd ;
    dct:created "2024-12-01"^^xsd:date ;
    rdfs:isDefinedBy ai-owl: ;
    rdfs:subClassOf ai-owl:BiometricIdentification ;
    sw:term_status "accepted"@en ;
    skos:definition "Capability involving biometric identification carried out locally"@en ;
    skos:prefLabel "Local Biometric Identification"@en .

ai-owl:LogicTechnique a rdfs:Class,
        owl:Class,
        ai-owl:Technique ;
    dct:contributor _:Ne8d6151e3d8047e6a947b3ec1a3830a1 ;
    dct:created "2024-12-01"^^xsd:date ;
    rdfs:isDefinedBy ai-owl: ;
    rdfs:subClassOf ai-owl:Technique ;
    sw:term_status "accepted"@en ;
    skos:definition "Refers to logic based techniques"@en ;
    skos:prefLabel "Logic Technique"@en .

ai-owl:LongShortTermMemory a rdfs:Class,
        owl:Class,
        ai-owl:Technique ;
    dct:contributor _:Ne8d6151e3d8047e6a947b3ec1a3830a1 ;
    dct:created "2024-12-01"^^xsd:date ;
    dct:source " 3.4.7"@en,
        "ISO/IEC 22989"@en ;
    rdfs:isDefinedBy ai-owl: ;
    rdfs:subClassOf ai-owl:NeuralNetwork ;
    sw:term_status "accepted"@en ;
    skos:definition "Type of recurrent neural network that processes sequential data with a satisfactory performance for both long and short span dependencies"@en ;
    skos:prefLabel "Long Short-Term Memory (LSTM)"@en .

ai-owl:MachineLearning a rdfs:Class,
        owl:Class,
        ai-owl:Technique ;
    dct:contributor _:Ne8d6151e3d8047e6a947b3ec1a3830a1 ;
    dct:created "2024-12-01"^^xsd:date ;
    dct:source " 3.3.5"@en,
        "ISO/IEC 22989:2022"@en ;
    rdfs:isDefinedBy ai-owl: ;
    rdfs:subClassOf ai-owl:Technique ;
    sw:term_status "accepted"@en ;
    skos:definition "Process of optimizing model parameters through computational techniques, such that the model's behaviour reflects the data or experience"@en ;
    skos:prefLabel "Machine Learning"@en .

ai-owl:MachineLearningModel a rdfs:Class,
        owl:Class ;
    dct:contributor _:Ne8d6151e3d8047e6a947b3ec1a3830a1 ;
    dct:created "2024-12-01"^^xsd:date ;
    dct:source " 3.3.7"@en,
        "ISO/IEC 22989:2022"@en ;
    rdfs:isDefinedBy ai-owl: ;
    rdfs:subClassOf ai-owl:Model ;
    sw:term_status "accepted"@en ;
    skos:definition "Mathematical construct that generates an inference or prediction  based on input data or information"@en ;
    skos:prefLabel "Machine Learning Model"@en .

ai-owl:MachineLearningPlatform a rdfs:Class,
        owl:Class,
        dpv-owl:Technology ;
    dct:contributor _:Ne8d6151e3d8047e6a947b3ec1a3830a1 ;
    dct:created "2024-12-01"^^xsd:date ;
    rdfs:isDefinedBy ai-owl: ;
    rdfs:subClassOf tech-owl:Platform ;
    sw:term_status "accepted"@en ;
    skos:definition "Technology platform for developing, deploying, and managing machine learning models and resources"@en ;
    skos:prefLabel "Machine Learning Platform"@en .

ai-owl:MachineTranslation a rdfs:Class,
        owl:Class,
        ai-owl:Capability ;
    dct:contributor _:Ne8d6151e3d8047e6a947b3ec1a3830a1 ;
    dct:created "2024-12-01"^^xsd:date ;
    dct:source " 3.6.5"@en,
        "ISO/IEC 22989:2022"@en ;
    rdfs:isDefinedBy ai-owl: ;
    rdfs:subClassOf ai-owl:LanguageCapability ;
    sw:term_status "accepted"@en ;
    skos:definition "Capability for automated translation of text or speech from one natural language to another using a computer system"@en ;
    skos:prefLabel "Machine Translation"@en .

ai-owl:Measure a rdfs:Class,
        owl:Class ;
    dct:created "2024-04-28"^^xsd:date ;
    rdfs:isDefinedBy ai-owl: ;
    rdfs:subClassOf dpv-owl:RiskMitigationMeasure ;
    sw:term_status "accepted"@en ;
    skos:definition "Measure to address risk associated with AI Systems"@en ;
    skos:prefLabel "Measure"@en ;
    skos:scopeNote "This concept is a stub"@en .

ai-owl:MissingFeaturesAndLabelsBias a rdfs:Class,
        owl:Class,
        dpv-owl:RiskConcept,
        risk-owl:PotentialRisk,
        risk-owl:PotentialRiskSource ;
    dct:contributor _:N606ea170c32e4fb5ac26e62242d8681b,
        _:Ne8d6151e3d8047e6a947b3ec1a3830a1 ;
    dct:created "2024-09-13"^^xsd:date ;
    dct:source "ISO/IEC 24027:2021"@en ;
    rdfs:isDefinedBy ai-owl: ;
    rdfs:subClassOf ai-owl:DataBias ;
    sw:term_status "accepted"@en ;
    skos:definition "Bias that occurs when features are missing from individual training samples"@en ;
    skos:prefLabel "Missing Features And Labels Bias"@en ;
    skos:scopeNote "If the frequency of missing features is higher for one group than another then this presents another vector for bias"@en .

ai-owl:Model a rdfs:Class,
        owl:Class ;
    dct:contributor _:Ne8d6151e3d8047e6a947b3ec1a3830a1 ;
    dct:created "2024-05-17"^^xsd:date ;
    dct:source " OECD"@en,
        "ISO/IEC 22989:2022"@en ;
    rdfs:isDefinedBy ai-owl: ;
    rdfs:subClassOf ai-owl:AI,
        tech-owl:Model ;
    sw:term_status "accepted"@en ;
    skos:definition "Physical, mathematical or otherwise logical representation of a system, entity, phenomenon, process or data involving the use of AI techniques"@en ;
    skos:prefLabel "Model"@en .

ai-owl:ModelBias a rdfs:Class,
        owl:Class,
        dpv-owl:RiskConcept,
        risk-owl:PotentialRisk,
        risk-owl:PotentialRiskSource ;
    dct:contributor _:N606ea170c32e4fb5ac26e62242d8681b,
        _:Ne8d6151e3d8047e6a947b3ec1a3830a1 ;
    dct:created "2024-09-13"^^xsd:date ;
    dct:source "ISO/IEC 24027:2021"@en ;
    rdfs:isDefinedBy ai-owl: ;
    rdfs:subClassOf ai-owl:EngineeringDecisionBias ;
    sw:term_status "accepted"@en ;
    skos:definition "Bias that occurs when ML uses functions like a maximum likelihood estimator to determine parameters, and there is data skew or under-representation present in the data, where the maximum likelihood estimation tends to amplify any underlying bias in the distribution"@en ;
    skos:prefLabel "Model Bias"@en .

ai-owl:ModelEvasion a rdfs:Class,
        owl:Class,
        dpv-owl:RiskConcept,
        risk-owl:IntegrityConcept,
        risk-owl:PotentialConsequence,
        risk-owl:PotentialRisk,
        risk-owl:PotentialRiskSource ;
    dct:contributor _:Ne8d6151e3d8047e6a947b3ec1a3830a1 ;
    dct:created "2024-12-01"^^xsd:date ;
    rdfs:isDefinedBy ai-owl: ;
    rdfs:subClassOf ai-owl:SecurityAttack ;
    sw:term_status "accepted"@en ;
    skos:definition "An input, which seems normal for a human but is wrongly classified by ML models"@en ;
    skos:prefLabel "Model Evasion"@en ;
    skos:scopeNote "(The EU Assessment List for Trustworthy AI (ALTAI),https://data.europa.eu/doi/10.2759/002360)"@en .

ai-owl:ModelExpressivenessBias a rdfs:Class,
        owl:Class,
        dpv-owl:RiskConcept,
        risk-owl:PotentialRisk,
        risk-owl:PotentialRiskSource ;
    dct:contributor _:N606ea170c32e4fb5ac26e62242d8681b,
        _:Ne8d6151e3d8047e6a947b3ec1a3830a1 ;
    dct:created "2024-09-13"^^xsd:date ;
    dct:source "ISO/IEC 24027:2021"@en ;
    rdfs:isDefinedBy ai-owl: ;
    rdfs:subClassOf ai-owl:ModelInteractionBias ;
    sw:term_status "accepted"@en ;
    skos:definition "Bias that occurs from the number and nature of parameters in a model as well as the neural network topology which affect the expressiveness of the model and any feature that affects model expressiveness differently across groups"@en ;
    skos:prefLabel "Model Expressiveness Bias"@en .

ai-owl:ModelInteractionBias a rdfs:Class,
        owl:Class,
        dpv-owl:RiskConcept,
        risk-owl:PotentialRisk,
        risk-owl:PotentialRiskSource ;
    dct:contributor _:N606ea170c32e4fb5ac26e62242d8681b,
        _:Ne8d6151e3d8047e6a947b3ec1a3830a1 ;
    dct:created "2024-09-13"^^xsd:date ;
    dct:source "ISO/IEC 24027:2021"@en ;
    rdfs:isDefinedBy ai-owl: ;
    rdfs:subClassOf ai-owl:EngineeringDecisionBias ;
    sw:term_status "accepted"@en ;
    skos:definition "Bias that occurs from the structure of a model to create biased predictions"@en ;
    skos:prefLabel "Model Interaction Bias"@en .

ai-owl:ModelInversion a rdfs:Class,
        owl:Class,
        dpv-owl:RiskConcept,
        risk-owl:ConfidentialityConcept,
        risk-owl:PotentialConsequence,
        risk-owl:PotentialRisk,
        risk-owl:PotentialRiskSource ;
    dct:contributor _:Ne8d6151e3d8047e6a947b3ec1a3830a1 ;
    dct:created "2024-12-01"^^xsd:date ;
    rdfs:isDefinedBy ai-owl: ;
    rdfs:subClassOf ai-owl:SecurityAttack ;
    sw:term_status "accepted"@en ;
    skos:definition "A type of attack to AI models, in which the access to a model is abused to infer information about the training data"@en ;
    skos:prefLabel "Model Inversion"@en ;
    skos:scopeNote "(HLEG Assessment List for Trustworthy Artificial Intelligence (ALTAI),https://digital-strategy.ec.europa.eu/en/library/assessment-list-trustworthy-artificial-intelligence-altai-self-assessment)"@en .

ai-owl:ModelRisk a rdfs:Class,
        owl:Class,
        dpv-owl:RiskConcept,
        risk-owl:PotentialRisk,
        risk-owl:PotentialRiskSource ;
    dct:contributor _:Ne8d6151e3d8047e6a947b3ec1a3830a1 ;
    dct:created "2024-12-01"^^xsd:date ;
    rdfs:isDefinedBy ai-owl: ;
    rdfs:subClassOf ai-owl:RiskConcept ;
    sw:term_status "accepted"@en ;
    skos:definition "Risks associated with AI Models"@en ;
    skos:prefLabel "Model Risk"@en .

ai-owl:MultiModalRetrieval a rdfs:Class,
        owl:Class,
        ai-owl:Capability ;
    dct:contributor _:N0a43dd9ea5e94fe695d8b7df8802cfdd ;
    dct:created "2024-12-01"^^xsd:date ;
    rdfs:isDefinedBy ai-owl: ;
    rdfs:subClassOf ai-owl:InformationRetrieval ;
    sw:term_status "accepted"@en ;
    skos:definition "Capability for retrieval of information using multiple modalities such as text, images, audio, and video and supporting cross-modal queries such as taking text as input to search images"@en ;
    skos:prefLabel "Multi-modal Retrieval"@en .

ai-owl:MusicInformationRetrieval a rdfs:Class,
        owl:Class,
        ai-owl:Capability ;
    dct:contributor _:Ne8d6151e3d8047e6a947b3ec1a3830a1 ;
    dct:created "2024-12-01"^^xsd:date ;
    dct:source " Defining Artificial Intelligence 2.0"@en,
        "AI Watch"@en ;
    rdfs:isDefinedBy ai-owl: ;
    rdfs:subClassOf ai-owl:InformationRetrieval ;
    sw:term_status "accepted"@en ;
    skos:definition "Capability for retrieving, analyzing, and categorizing music-related information such as audio files, melodies, or lyrics using audio features, metadata, and user queries"@en ;
    skos:prefLabel "Music Information Retrieval (MIR)"@en .

ai-owl:NamedEntityRecognition a rdfs:Class,
        owl:Class,
        ai-owl:Capability ;
    dct:contributor _:Ne8d6151e3d8047e6a947b3ec1a3830a1 ;
    dct:created "2024-12-01"^^xsd:date ;
    dct:source " 3.6.6"@en,
        "ISO/IEC 22989:2022"@en ;
    rdfs:isDefinedBy ai-owl: ;
    rdfs:subClassOf ai-owl:LanguageCapability ;
    sw:term_status "accepted"@en ;
    skos:definition "Capability for recognizing and labelling the denotational names of entities and their categories for sequences of words in a stream of text or speech"@en ;
    skos:prefLabel "Named Entity Recognition"@en .

ai-owl:NarrowAI a rdfs:Class,
        owl:Class ;
    dct:contributor _:Ne8d6151e3d8047e6a947b3ec1a3830a1 ;
    dct:created "2024-12-01"^^xsd:date ;
    dct:source " 3.1.24"@en,
        "ISO/IEC 22989:2022"@en ;
    rdfs:isDefinedBy ai-owl: ;
    rdfs:subClassOf ai-owl:AISystem ;
    sw:term_status "accepted"@en ;
    skos:definition "Type of AI system that is focused on defined tasks to address a specific problem i.e. it addresses a narrow scope of tasks and problems"@en ;
    skos:prefLabel "Narrow AI"@en .

ai-owl:NaturalLanguageGeneration a rdfs:Class,
        owl:Class,
        ai-owl:Capability ;
    dct:contributor _:Ne8d6151e3d8047e6a947b3ec1a3830a1 ;
    dct:created "2024-12-01"^^xsd:date ;
    dct:source " 3.6.8"@en,
        "ISO/IEC 22989:2022"@en ;
    rdfs:isDefinedBy ai-owl: ;
    rdfs:subClassOf ai-owl:LanguageCapability ;
    sw:term_status "accepted"@en ;
    skos:definition "Converting data carrying semantics into natural language"@en ;
    skos:prefLabel "Natural Language Generation"@en .

ai-owl:NeuralNetwork a rdfs:Class,
        owl:Class,
        ai-owl:Technique ;
    dct:contributor _:Ne8d6151e3d8047e6a947b3ec1a3830a1 ;
    dct:created "2024-12-01"^^xsd:date ;
    dct:source " 3.4.8"@en,
        "ISO/IEC 22989"@en ;
    rdfs:isDefinedBy ai-owl: ;
    rdfs:subClassOf ai-owl:MachineLearning ;
    sw:term_status "accepted"@en ;
    skos:definition "Network of one or more layers of neurons connected by weighted links with adjustable weights, which takes input data and produces an output"@en ;
    skos:prefLabel "Neural Network"@en .

ai-owl:NonRepresentativeSamplingBias a rdfs:Class,
        owl:Class,
        dpv-owl:RiskConcept,
        risk-owl:PotentialRisk,
        risk-owl:PotentialRiskSource ;
    dct:contributor _:N606ea170c32e4fb5ac26e62242d8681b,
        _:Ne8d6151e3d8047e6a947b3ec1a3830a1 ;
    dct:created "2024-09-13"^^xsd:date ;
    dct:source "ISO/IEC 24027:2021"@en ;
    rdfs:isDefinedBy ai-owl: ;
    rdfs:subClassOf ai-owl:DataBias ;
    sw:term_status "accepted"@en ;
    skos:definition "Bias that occurs if a dataset is not representative of the intended deployment environment, where the model learns biases based on the ways in which the data is non-representative"@en ;
    skos:prefLabel "Non-Representative Sampling Bias"@en .

ai-owl:ObjectRecognition a rdfs:Class,
        owl:Class,
        ai-owl:Capability ;
    dct:contributor _:Ne8d6151e3d8047e6a947b3ec1a3830a1 ;
    dct:created "2024-12-01"^^xsd:date ;
    dct:source " Defining Artificial Intelligence 2.0"@en,
        "AI Watch"@en ;
    rdfs:isDefinedBy ai-owl: ;
    rdfs:subClassOf ai-owl:ComputerVision ;
    sw:term_status "accepted"@en ;
    skos:definition "Capability to recognise objects"@en ;
    skos:prefLabel "Object Recognition"@en .

ai-owl:OperationStage a rdfs:Class,
        owl:Class,
        ai-owl:LifecycleStage ;
    dct:contributor _:Ne8d6151e3d8047e6a947b3ec1a3830a1 ;
    dct:created "2024-12-01"^^xsd:date ;
    dct:source "ISO/IEC 22989:2028"@en ;
    rdfs:isDefinedBy ai-owl: ;
    rdfs:subClassOf ai-owl:LifecycleStage ;
    sw:term_status "accepted"@en ;
    skos:definition "The stage in the lifecycle where an AI system is running and generally available for operations"@en ;
    skos:prefLabel "Operation Stage"@en .

ai-owl:OptimisationMethod a rdfs:Class,
        owl:Class,
        ai-owl:Technique ;
    dct:contributor _:Ne8d6151e3d8047e6a947b3ec1a3830a1 ;
    dct:created "2024-12-01"^^xsd:date ;
    rdfs:isDefinedBy ai-owl: ;
    rdfs:subClassOf ai-owl:StatisticalTechnique ;
    sw:term_status "accepted"@en ;
    skos:definition "Refers to optimisation Method"@en ;
    skos:prefLabel "Optimisation Method"@en .

ai-owl:PartOfSpeechTagging a rdfs:Class,
        owl:Class,
        ai-owl:Capability ;
    dct:contributor _:Ne8d6151e3d8047e6a947b3ec1a3830a1 ;
    dct:created "2024-12-01"^^xsd:date ;
    dct:source " 3.6.13"@en,
        "ISO/IEC 22989:2022"@en ;
    rdfs:isDefinedBy ai-owl: ;
    rdfs:subClassOf ai-owl:LanguageCapability ;
    sw:term_status "accepted"@en ;
    skos:definition "Capability for assigning a category (e.g. verb, noun, adjective) to a word based on its grammatical properties"@en ;
    skos:prefLabel "Part Of Speech Tagging"@en .

ai-owl:PersonalityTraitAnalysis a rdfs:Class,
        owl:Class,
        ai-owl:Capability ;
    dct:contributor _:Ne8d6151e3d8047e6a947b3ec1a3830a1 ;
    dct:created "2024-12-01"^^xsd:date ;
    rdfs:isDefinedBy ai-owl: ;
    rdfs:subClassOf ai-owl:HumanOrientedCapability ;
    sw:term_status "accepted"@en ;
    skos:definition "Capability for determining and analysing people's personality traits"@en ;
    skos:prefLabel "Personality Trait Analysis"@en .

ai-owl:PostTimeBiometricIdentification a rdfs:Class,
        owl:Class,
        ai-owl:Capability ;
    dct:contributor _:N0a43dd9ea5e94fe695d8b7df8802cfdd ;
    dct:created "2024-12-01"^^xsd:date ;
    rdfs:isDefinedBy ai-owl: ;
    rdfs:subClassOf ai-owl:BiometricIdentification ;
    sw:term_status "accepted"@en ;
    skos:definition "Capability involving biometric identification carried out later or not in real-time or not-instaneously"@en ;
    skos:prefLabel "Post-Time Biometric Identification"@en .

ai-owl:Profiling a rdfs:Class,
        owl:Class,
        ai-owl:Capability ;
    dct:contributor _:Ne8d6151e3d8047e6a947b3ec1a3830a1 ;
    dct:created "2024-12-01"^^xsd:date ;
    rdfs:isDefinedBy ai-owl: ;
    rdfs:subClassOf ai-owl:HumanOrientedCapability,
        dpv-owl:Profiling ;
    sw:term_status "accepted"@en ;
    skos:definition "Capability where AI is used to construct a profile of an individual (human) or a group of individuals"@en ;
    skos:prefLabel "Profiling"@en .

ai-owl:QuestionAnswering a rdfs:Class,
        owl:Class,
        ai-owl:Capability ;
    dct:contributor _:Ne8d6151e3d8047e6a947b3ec1a3830a1 ;
    dct:created "2024-12-01"^^xsd:date ;
    dct:source " 3.6.14"@en,
        "ISO/IEC IEC 22989:2022"@en ;
    rdfs:isDefinedBy ai-owl: ;
    rdfs:subClassOf ai-owl:LanguageCapability ;
    sw:term_status "accepted"@en ;
    skos:definition "Capability for determining the most appropriate answer to a question provided in natural language"@en ;
    skos:prefLabel "Question Answering"@en .

ai-owl:RealTimeBiometricIdentification a rdfs:Class,
        owl:Class,
        ai-owl:Capability ;
    dct:contributor _:Ne8d6151e3d8047e6a947b3ec1a3830a1 ;
    dct:created "2024-12-01"^^xsd:date ;
    rdfs:isDefinedBy ai-owl: ;
    rdfs:subClassOf ai-owl:BiometricIdentification ;
    sw:term_status "accepted"@en ;
    skos:definition "Capability involving biometric identification carried out in real-time or instataneously"@en ;
    skos:prefLabel "Real-Time Biometric Identification"@en .

ai-owl:ReasoningTechnique a rdfs:Class,
        owl:Class,
        ai-owl:Technique ;
    dct:contributor _:Ne8d6151e3d8047e6a947b3ec1a3830a1 ;
    dct:created "2024-12-01"^^xsd:date ;
    rdfs:isDefinedBy ai-owl: ;
    rdfs:subClassOf ai-owl:Technique ;
    sw:term_status "accepted"@en ;
    skos:definition "Refers to reasoning techniques"@en ;
    skos:prefLabel "Reasoning Technique"@en .

ai-owl:RecurrentNeuralNetwork a rdfs:Class,
        owl:Class,
        ai-owl:Technique ;
    dct:contributor _:Ne8d6151e3d8047e6a947b3ec1a3830a1 ;
    dct:created "2024-12-01"^^xsd:date ;
    dct:source " 3.4.10"@en,
        "ISO/IEC 22989"@en ;
    rdfs:isDefinedBy ai-owl: ;
    rdfs:subClassOf ai-owl:NeuralNetwork ;
    sw:term_status "accepted"@en ;
    skos:definition "Neural network in which outputs from both the previous layer and the previous processing step are fed into the current layer"@en ;
    skos:prefLabel "Recurrent Neural Network (RNN)"@en .

ai-owl:ReevaluationStage a rdfs:Class,
        owl:Class,
        ai-owl:LifecycleStage ;
    dct:contributor _:Ne8d6151e3d8047e6a947b3ec1a3830a1 ;
    dct:created "2024-12-01"^^xsd:date ;
    dct:source "ISO/IEC 22989:2033"@en ;
    rdfs:isDefinedBy ai-owl: ;
    rdfs:subClassOf ai-owl:LifecycleStage ;
    sw:term_status "accepted"@en ;
    skos:definition "The stage in the lifecycle where the AI system is reevaluated after the operation and monitoring stage based on the operations of the AI system"@en ;
    skos:prefLabel "Reevaluation Stage"@en .

ai-owl:ReinforcementLearning a rdfs:Class,
        owl:Class,
        ai-owl:Technique ;
    dct:contributor _:Ne8d6151e3d8047e6a947b3ec1a3830a1 ;
    dct:created "2024-12-01"^^xsd:date ;
    dct:source " 3.3.9"@en,
        "ISO/IEC 22989:2022"@en ;
    rdfs:isDefinedBy ai-owl: ;
    rdfs:subClassOf ai-owl:MachineLearning ;
    sw:term_status "accepted"@en ;
    skos:definition "Learning of an optimal sequence of actions to maximize a reward through interaction with an environment"@en ;
    skos:prefLabel "Reinforcement Learning"@en .

ai-owl:RelationshipExtraction a rdfs:Class,
        owl:Class,
        ai-owl:Capability ;
    dct:contributor _:Ne8d6151e3d8047e6a947b3ec1a3830a1 ;
    dct:created "2024-12-01"^^xsd:date ;
    dct:source " 3.6.15"@en,
        "ISO/IEC 22989:2022"@en ;
    rdfs:isDefinedBy ai-owl: ;
    rdfs:subClassOf ai-owl:LanguageCapability ;
    sw:term_status "accepted"@en ;
    skos:definition "Capability for identifying relationships among entities mentioned in a text"@en ;
    skos:prefLabel "Relationship Extraction"@en .

ai-owl:RemoteBiometricIdentification a rdfs:Class,
        owl:Class,
        ai-owl:Capability ;
    dct:contributor _:Ne8d6151e3d8047e6a947b3ec1a3830a1 ;
    dct:created "2024-12-01"^^xsd:date ;
    rdfs:isDefinedBy ai-owl: ;
    rdfs:subClassOf ai-owl:BiometricIdentification ;
    sw:term_status "accepted"@en ;
    skos:definition "Capability involving biometric identification carried out remotely"@en ;
    skos:prefLabel "Remote Biometric Identification"@en .

ai-owl:RepairStage a rdfs:Class,
        owl:Class,
        ai-owl:LifecycleStage ;
    dct:contributor _:N0a43dd9ea5e94fe695d8b7df8802cfdd ;
    dct:created "2024-12-01"^^xsd:date ;
    dct:source "ISO/IEC 22989:2030"@en ;
    rdfs:isDefinedBy ai-owl: ;
    rdfs:subClassOf ai-owl:OperationStage ;
    sw:term_status "accepted"@en ;
    skos:definition "The stage in the lifecycle where  an AI system is being repaired due to suspected or occured incidents"@en ;
    skos:prefLabel "Repair Stage"@en .

ai-owl:ReplaceStage a rdfs:Class,
        owl:Class,
        ai-owl:LifecycleStage ;
    dct:contributor _:N0a43dd9ea5e94fe695d8b7df8802cfdd ;
    dct:created "2024-12-01"^^xsd:date ;
    dct:source "ISO/IEC 22989:2037"@en ;
    rdfs:isDefinedBy ai-owl: ;
    rdfs:subClassOf ai-owl:RetirementStage ;
    sw:term_status "accepted"@en ;
    skos:definition "The stage in the lifecycle where the AI system is being replaced as part of retirement"@en ;
    skos:prefLabel "Replace Stage"@en .

ai-owl:RetirementStage a rdfs:Class,
        owl:Class,
        ai-owl:LifecycleStage ;
    dct:contributor _:Ne8d6151e3d8047e6a947b3ec1a3830a1 ;
    dct:created "2024-12-01"^^xsd:date ;
    dct:source "ISO/IEC 22989:2034"@en ;
    rdfs:isDefinedBy ai-owl: ;
    rdfs:subClassOf ai-owl:LifecycleStage ;
    sw:term_status "accepted"@en ;
    skos:definition "The stage in the lifecycle where the AI system is retired and becomes obsolete"@en ;
    skos:prefLabel "Retirement Stage"@en .

ai-owl:RiskConcept a rdfs:Class,
        owl:Class,
        risk-owl:PotentialRisk,
        risk-owl:PotentialRiskSource ;
    dct:contributor _:Ne8d6151e3d8047e6a947b3ec1a3830a1 ;
    dct:created "2024-04-28"^^xsd:date ;
    rdfs:isDefinedBy ai-owl: ;
    rdfs:subClassOf dpv-owl:RiskConcept ;
    sw:term_status "accepted"@en ;
    skos:definition "Risk concepts such as risk sources, risks, consequences, and impacts associated specifically with development, use, or operation of AI"@en ;
    skos:prefLabel "RiskConcept"@en .

ai-owl:Robot a rdfs:Class,
        owl:Class ;
    dct:contributor _:Ne8d6151e3d8047e6a947b3ec1a3830a1 ;
    dct:created "2024-12-01"^^xsd:date ;
    dct:source " 3.1.29"@en,
        "ISO/IEC 22989:2022"@en ;
    rdfs:isDefinedBy ai-owl: ;
    rdfs:subClassOf ai-owl:AISystem ;
    sw:term_status "accepted"@en ;
    skos:definition "An automation system with actuators that performs intended tasks in the physical world, by means of sensing its environment and a software control system"@en ;
    skos:prefLabel "Robot"@en .

ai-owl:SearchMethod a rdfs:Class,
        owl:Class,
        ai-owl:Technique ;
    dct:contributor _:Ne8d6151e3d8047e6a947b3ec1a3830a1 ;
    dct:created "2024-12-01"^^xsd:date ;
    rdfs:isDefinedBy ai-owl: ;
    rdfs:subClassOf ai-owl:StatisticalTechnique ;
    sw:term_status "accepted"@en ;
    skos:definition "Refers to statistical-based search Methods"@en ;
    skos:prefLabel "Search Method"@en .

ai-owl:SecurityAttack a rdfs:Class,
        owl:Class,
        dpv-owl:RiskConcept,
        risk-owl:PotentialRisk,
        risk-owl:PotentialRiskSource ;
    dct:contributor _:Ne8d6151e3d8047e6a947b3ec1a3830a1 ;
    dct:created "2024-12-01"^^xsd:date ;
    rdfs:isDefinedBy ai-owl: ;
    rdfs:subClassOf ai-owl:RiskConcept ;
    sw:term_status "accepted"@en ;
    skos:definition "Risks or issues associated with security attacks related to AI technologies, models, and systems"@en ;
    skos:prefLabel "Security Attack"@en .

ai-owl:SemiSupervisedLearning a rdfs:Class,
        owl:Class,
        ai-owl:Technique ;
    dct:contributor _:Ne8d6151e3d8047e6a947b3ec1a3830a1 ;
    dct:created "2024-12-01"^^xsd:date ;
    dct:source " 3.3.11"@en,
        "ISO/IEC 22989:2022"@en ;
    rdfs:isDefinedBy ai-owl: ;
    rdfs:subClassOf ai-owl:MachineLearning ;
    sw:term_status "accepted"@en ;
    skos:definition "Machine learning that makes use of both labelled and unlabelled data during training"@en ;
    skos:prefLabel "Semi Supervised Learning"@en .

ai-owl:SentimentAnalysis a rdfs:Class,
        owl:Class,
        ai-owl:Capability ;
    dct:contributor _:Ne8d6151e3d8047e6a947b3ec1a3830a1 ;
    dct:created "2024-12-01"^^xsd:date ;
    dct:source " 3.6.16"@en,
        "ISO/IEC 22989:2022"@en ;
    rdfs:isDefinedBy ai-owl: ;
    rdfs:subClassOf ai-owl:HumanOrientedCapability,
        ai-owl:LanguageCapability ;
    sw:term_status "accepted"@en ;
    skos:definition "Capability for computationally identifying and categorizing opinions expressed in a piece of text, speech or image, to determine a range of feeling such as from positive to negative"@en ;
    skos:prefLabel "Sentiment Analysis"@en .

ai-owl:ServiceRobot a rdfs:Class,
        owl:Class ;
    dct:contributor _:Ne8d6151e3d8047e6a947b3ec1a3830a1 ;
    dct:created "2024-12-01"^^xsd:date ;
    dct:source " 3.1.29"@en,
        " 3.7"@en,
        " ISO 8373:2021"@en,
        "ISO/IEC 22989:2022"@en ;
    rdfs:isDefinedBy ai-owl: ;
    rdfs:subClassOf ai-owl:Robot ;
    sw:term_status "accepted"@en ;
    skos:definition "A robot or robotic system in personal use or professional use that performs useful tasks for humans or equipment"@en ;
    skos:prefLabel "Service Robot"@en .

ai-owl:SocialRobot a rdfs:Class,
        owl:Class ;
    dct:contributor _:Ne8d6151e3d8047e6a947b3ec1a3830a1 ;
    dct:created "2024-12-01"^^xsd:date ;
    dct:source " Defining Artificial Intelligence 2.0"@en,
        "AI Watch"@en ;
    rdfs:isDefinedBy ai-owl: ;
    rdfs:subClassOf ai-owl:Robot ;
    sw:term_status "accepted"@en ;
    skos:definition "A robot or robotic system with social interaction functions"@en ;
    skos:prefLabel "Social Robot"@en .

ai-owl:SoundSourceSeparation a rdfs:Class,
        owl:Class,
        ai-owl:Capability ;
    dct:contributor _:Ne8d6151e3d8047e6a947b3ec1a3830a1 ;
    dct:created "2024-12-01"^^xsd:date ;
    dct:source " Defining Artificial Intelligence 2.0"@en,
        "AI Watch"@en ;
    rdfs:isDefinedBy ai-owl: ;
    rdfs:subClassOf ai-owl:AudioCapability ;
    sw:term_status "accepted"@en ;
    skos:definition "Capability for extracting individual sound from audio recordings"@en ;
    skos:prefLabel "Sound Source Separation"@en .

ai-owl:SoundSynthesis a rdfs:Class,
        owl:Class,
        ai-owl:Capability ;
    dct:contributor _:Ne8d6151e3d8047e6a947b3ec1a3830a1 ;
    dct:created "2024-12-01"^^xsd:date ;
    dct:source " Defining Artificial Intelligence 2.0"@en,
        "AI Watch"@en ;
    rdfs:isDefinedBy ai-owl: ;
    rdfs:subClassOf ai-owl:AudioCapability,
        ai-owl:ContentGeneration ;
    sw:term_status "accepted"@en ;
    skos:definition "Capability for generation of artificial sound"@en ;
    skos:prefLabel "Sound Synthesis"@en .

ai-owl:SpeakerRecognition a rdfs:Class,
        owl:Class,
        ai-owl:Capability ;
    dct:contributor _:Ne8d6151e3d8047e6a947b3ec1a3830a1 ;
    dct:created "2024-12-01"^^xsd:date ;
    dct:source " Defining Artificial Intelligence 2.0"@en,
        "AI Watch"@en ;
    rdfs:isDefinedBy ai-owl: ;
    rdfs:subClassOf ai-owl:AudioProcessing,
        ai-owl:HumanOrientedCapability ;
    sw:term_status "accepted"@en ;
    skos:definition "Capability of recognising speaker(s) in audio recordings"@en ;
    skos:prefLabel "Speaker Recognition"@en .

ai-owl:SpeechRecognition a rdfs:Class,
        owl:Class,
        ai-owl:Capability ;
    dct:contributor _:Ne8d6151e3d8047e6a947b3ec1a3830a1 ;
    dct:created "2024-12-01"^^xsd:date ;
    dct:source " 3.6.17"@en,
        "ISO/IEC 22989:2022"@en ;
    rdfs:isDefinedBy ai-owl: ;
    rdfs:subClassOf ai-owl:AudioProcessing,
        ai-owl:HumanOrientedCapability ;
    sw:term_status "accepted"@en ;
    skos:definition "Capability of converting a speech signal to a representation of the content of the speech"@en ;
    skos:prefLabel "Speech Recognition"@en .

ai-owl:SpeechSynthesis a rdfs:Class,
        owl:Class,
        ai-owl:Capability ;
    dct:contributor _:Ne8d6151e3d8047e6a947b3ec1a3830a1 ;
    dct:created "2024-12-01"^^xsd:date ;
    dct:source " 3.6.18"@en,
        "ISO/IEC 22989:2022"@en ;
    rdfs:isDefinedBy ai-owl: ;
    rdfs:subClassOf ai-owl:AudioCapability,
        ai-owl:ContentGeneration ;
    sw:term_status "accepted"@en ;
    skos:definition "Capability for generation of artificial speech"@en ;
    skos:prefLabel "Speech Synthesis"@en .

ai-owl:StatisticalTechnique a rdfs:Class,
        owl:Class,
        ai-owl:Technique ;
    dct:contributor _:Ne8d6151e3d8047e6a947b3ec1a3830a1 ;
    dct:created "2024-12-01"^^xsd:date ;
    rdfs:isDefinedBy ai-owl: ;
    rdfs:subClassOf ai-owl:Technique ;
    sw:term_status "accepted"@en ;
    skos:definition "Refers to techniques that are based on statistics"@en ;
    skos:prefLabel "Statistical Technique"@en .

ai-owl:SupervisedLearning a rdfs:Class,
        owl:Class,
        ai-owl:Technique ;
    dct:contributor _:Ne8d6151e3d8047e6a947b3ec1a3830a1 ;
    dct:created "2024-12-01"^^xsd:date ;
    dct:source " 3.3.11"@en,
        "ISO/IEC 22989:2022"@en ;
    rdfs:isDefinedBy ai-owl: ;
    rdfs:subClassOf ai-owl:MachineLearning ;
    sw:term_status "accepted"@en ;
    skos:definition "Machine learning that makes only use of labelled data during training"@en ;
    skos:prefLabel "Supervised Learning"@en .

ai-owl:SupportVectorMachine a rdfs:Class,
        owl:Class,
        ai-owl:Technique ;
    dct:contributor _:Ne8d6151e3d8047e6a947b3ec1a3830a1 ;
    dct:created "2024-12-01"^^xsd:date ;
    dct:source " 3.3.13"@en,
        "ISO/IEC 22989"@en ;
    rdfs:isDefinedBy ai-owl: ;
    rdfs:subClassOf ai-owl:MachineLearning ;
    sw:term_status "accepted"@en ;
    skos:definition "A machine learning algorithm that finds decision boundaries with maximal margins"@en ;
    skos:prefLabel "Support Vector Machine"@en .

ai-owl:SymbolicReasoning a rdfs:Class,
        owl:Class,
        ai-owl:Technique ;
    dct:contributor _:Ne8d6151e3d8047e6a947b3ec1a3830a1 ;
    dct:created "2024-12-01"^^xsd:date ;
    rdfs:isDefinedBy ai-owl: ;
    rdfs:subClassOf ai-owl:KnowledgeTechnique ;
    sw:term_status "accepted"@en ;
    skos:definition "Reasoning based on the knowledge encoded in a formal language"@en ;
    skos:prefLabel "Symbolic Reasoning"@en .

ai-owl:Technique a rdfs:Class,
        owl:Class ;
    dct:contributor _:Ne8d6151e3d8047e6a947b3ec1a3830a1 ;
    dct:created "2024-04-28"^^xsd:date ;
    rdfs:isDefinedBy ai-owl: ;
    rdfs:subClassOf ai-owl:AI ;
    sw:term_status "accepted"@en ;
    skos:definition "The underlying technological algorithm, method, or process that forms the technique for using or applying AI"@en ;
    skos:prefLabel "Technique"@en ;
    skos:scopeNote "This concept refers to the foundational computational implementation and is necessary to distinguish the 'algorithm' (ai:Technique) from the 'application' (ai:Capability) and 'goal' (dpv:Purpose)"@en .

ai-owl:TestingData a rdfs:Class,
        owl:Class ;
    dct:contributor _:Ne8d6151e3d8047e6a947b3ec1a3830a1 ;
    dct:created "2024-12-01"^^xsd:date ;
    rdfs:isDefinedBy ai-owl: ;
    rdfs:subClassOf ai-owl:Data ;
    sw:term_status "accepted"@en ;
    skos:definition "Data involved in the testing of an AI system or model"@en ;
    skos:prefLabel "Testing Data"@en .

ai-owl:TestingDataBias a rdfs:Class,
        owl:Class,
        dpv-owl:RiskConcept,
        risk-owl:PotentialRisk,
        risk-owl:PotentialRiskSource ;
    dct:contributor _:Ne8d6151e3d8047e6a947b3ec1a3830a1 ;
    dct:created "2024-12-01"^^xsd:date ;
    rdfs:isDefinedBy ai-owl: ;
    rdfs:subClassOf ai-owl:TestingDataRisk ;
    sw:term_status "accepted"@en ;
    skos:definition "Concept representing testing data containing or potentially containing bias"@en ;
    skos:prefLabel "Testing Data Bias"@en .

ai-owl:TestingDataInaccurate a rdfs:Class,
        owl:Class,
        dpv-owl:RiskConcept,
        risk-owl:PotentialRisk,
        risk-owl:PotentialRiskSource ;
    dct:contributor _:Ne8d6151e3d8047e6a947b3ec1a3830a1 ;
    dct:created "2024-12-01"^^xsd:date ;
    rdfs:isDefinedBy ai-owl: ;
    rdfs:subClassOf ai-owl:TestingDataRisk ;
    sw:term_status "accepted"@en ;
    skos:definition "Concept representing testing data being inaccurate"@en ;
    skos:prefLabel "Testing Data Inaccurate"@en .

ai-owl:TestingDataInappropriate a rdfs:Class,
        owl:Class,
        dpv-owl:RiskConcept,
        risk-owl:PotentialRisk,
        risk-owl:PotentialRiskSource ;
    dct:contributor _:Ne8d6151e3d8047e6a947b3ec1a3830a1 ;
    dct:created "2024-12-01"^^xsd:date ;
    rdfs:isDefinedBy ai-owl: ;
    rdfs:subClassOf ai-owl:TestingDataRisk ;
    sw:term_status "accepted"@en ;
    skos:definition "Concept representing testing data being inappropriate"@en ;
    skos:prefLabel "Testing Data Inappropriate"@en .

ai-owl:TestingDataIncomplete a rdfs:Class,
        owl:Class,
        dpv-owl:RiskConcept,
        risk-owl:PotentialRisk,
        risk-owl:PotentialRiskSource ;
    dct:contributor _:Ne8d6151e3d8047e6a947b3ec1a3830a1 ;
    dct:created "2024-12-01"^^xsd:date ;
    rdfs:isDefinedBy ai-owl: ;
    rdfs:subClassOf ai-owl:TestingDataRisk ;
    sw:term_status "accepted"@en ;
    skos:definition "Concept representing testing data being incomplete"@en ;
    skos:prefLabel "Testing Data Incomplete"@en .

ai-owl:TestingDataInconsistent a rdfs:Class,
        owl:Class,
        dpv-owl:RiskConcept,
        risk-owl:PotentialRisk,
        risk-owl:PotentialRiskSource ;
    dct:contributor _:Ne8d6151e3d8047e6a947b3ec1a3830a1 ;
    dct:created "2024-12-01"^^xsd:date ;
    rdfs:isDefinedBy ai-owl: ;
    rdfs:subClassOf ai-owl:TestingDataRisk ;
    sw:term_status "accepted"@en ;
    skos:definition "Concept representing testing data being inconsistent"@en ;
    skos:prefLabel "Testing Data Inconsistent"@en .

ai-owl:TestingDataMisclassified a rdfs:Class,
        owl:Class,
        dpv-owl:RiskConcept,
        risk-owl:PotentialRisk,
        risk-owl:PotentialRiskSource ;
    dct:contributor _:Ne8d6151e3d8047e6a947b3ec1a3830a1 ;
    dct:created "2024-12-01"^^xsd:date ;
    rdfs:isDefinedBy ai-owl: ;
    rdfs:subClassOf ai-owl:TestingDataRisk ;
    sw:term_status "accepted"@en ;
    skos:definition "Concept representing testing data being misclassified"@en ;
    skos:prefLabel "Testing Data Misclassified"@en .

ai-owl:TestingDataMisinterpretation a rdfs:Class,
        owl:Class,
        dpv-owl:RiskConcept,
        risk-owl:PotentialRisk,
        risk-owl:PotentialRiskSource ;
    dct:contributor _:Ne8d6151e3d8047e6a947b3ec1a3830a1 ;
    dct:created "2024-12-01"^^xsd:date ;
    rdfs:isDefinedBy ai-owl: ;
    rdfs:subClassOf ai-owl:TestingDataRisk ;
    sw:term_status "accepted"@en ;
    skos:definition "Concept representing testing data being misinterpretation"@en ;
    skos:prefLabel "Testing Data Misinterpretation"@en .

ai-owl:TestingDataNoise a rdfs:Class,
        owl:Class,
        dpv-owl:RiskConcept,
        risk-owl:PotentialRisk,
        risk-owl:PotentialRiskSource ;
    dct:contributor _:Ne8d6151e3d8047e6a947b3ec1a3830a1 ;
    dct:created "2024-12-01"^^xsd:date ;
    rdfs:isDefinedBy ai-owl: ;
    rdfs:subClassOf ai-owl:TestingDataRisk ;
    sw:term_status "accepted"@en ;
    skos:definition "Concept representing testing data being noise"@en ;
    skos:prefLabel "Testing Data Noise"@en .

ai-owl:TestingDataOutdated a rdfs:Class,
        owl:Class,
        dpv-owl:RiskConcept,
        risk-owl:PotentialRisk,
        risk-owl:PotentialRiskSource ;
    dct:contributor _:Ne8d6151e3d8047e6a947b3ec1a3830a1 ;
    dct:created "2024-12-01"^^xsd:date ;
    rdfs:isDefinedBy ai-owl: ;
    rdfs:subClassOf ai-owl:TestingDataRisk ;
    sw:term_status "accepted"@en ;
    skos:definition "Concept representing testing data being outdated"@en ;
    skos:prefLabel "Testing Data Outdated"@en .

ai-owl:TestingDataRisk a rdfs:Class,
        owl:Class,
        dpv-owl:RiskConcept,
        risk-owl:PotentialRisk,
        risk-owl:PotentialRiskSource ;
    dct:contributor _:Ne8d6151e3d8047e6a947b3ec1a3830a1 ;
    dct:created "2024-12-01"^^xsd:date ;
    rdfs:isDefinedBy ai-owl: ;
    rdfs:subClassOf ai-owl:DataRisk ;
    sw:term_status "accepted"@en ;
    skos:definition "Risks and risk concepts related to testing data"@en ;
    skos:prefLabel "Testing Data Risk"@en .

ai-owl:TestingDataSelectionError a rdfs:Class,
        owl:Class,
        dpv-owl:RiskConcept,
        risk-owl:PotentialRisk,
        risk-owl:PotentialRiskSource ;
    dct:contributor _:Ne8d6151e3d8047e6a947b3ec1a3830a1 ;
    dct:created "2024-12-01"^^xsd:date ;
    rdfs:isDefinedBy ai-owl: ;
    rdfs:subClassOf ai-owl:TestingDataRisk ;
    sw:term_status "accepted"@en ;
    skos:definition "Concept representing an error in testing data selection"@en ;
    skos:prefLabel "Testing Data Selection Error"@en .

ai-owl:TestingDataSparse a rdfs:Class,
        owl:Class,
        dpv-owl:RiskConcept,
        risk-owl:PotentialRisk,
        risk-owl:PotentialRiskSource ;
    dct:contributor _:Ne8d6151e3d8047e6a947b3ec1a3830a1 ;
    dct:created "2024-12-01"^^xsd:date ;
    rdfs:isDefinedBy ai-owl: ;
    rdfs:subClassOf ai-owl:TestingDataRisk ;
    sw:term_status "accepted"@en ;
    skos:definition "Concept representing testing data being sparse"@en ;
    skos:prefLabel "Testing Data Sparse"@en .

ai-owl:TestingDataUnrepresentative a rdfs:Class,
        owl:Class,
        dpv-owl:RiskConcept,
        risk-owl:PotentialRisk,
        risk-owl:PotentialRiskSource ;
    dct:contributor _:Ne8d6151e3d8047e6a947b3ec1a3830a1 ;
    dct:created "2024-12-01"^^xsd:date ;
    rdfs:isDefinedBy ai-owl: ;
    rdfs:subClassOf ai-owl:TestingDataRisk ;
    sw:term_status "accepted"@en ;
    skos:definition "Concept representing testing data being unrepresentative"@en ;
    skos:prefLabel "Testing Data Unrepresentative"@en .

ai-owl:TestingDataUnstructured a rdfs:Class,
        owl:Class,
        dpv-owl:RiskConcept,
        risk-owl:PotentialRisk,
        risk-owl:PotentialRiskSource ;
    dct:contributor _:Ne8d6151e3d8047e6a947b3ec1a3830a1 ;
    dct:created "2024-12-01"^^xsd:date ;
    rdfs:isDefinedBy ai-owl: ;
    rdfs:subClassOf ai-owl:TestingDataRisk ;
    sw:term_status "accepted"@en ;
    skos:definition "Concept representing testing data being unstructured"@en ;
    skos:prefLabel "Testing Data Unstructured"@en .

ai-owl:TestingDataUnverified a rdfs:Class,
        owl:Class,
        dpv-owl:RiskConcept,
        risk-owl:PotentialRisk,
        risk-owl:PotentialRiskSource ;
    dct:contributor _:Ne8d6151e3d8047e6a947b3ec1a3830a1 ;
    dct:created "2024-12-01"^^xsd:date ;
    rdfs:isDefinedBy ai-owl: ;
    rdfs:subClassOf ai-owl:TestingDataRisk ;
    sw:term_status "accepted"@en ;
    skos:definition "Concept representing testing data being unverified"@en ;
    skos:prefLabel "Testing Data Unverified"@en .

ai-owl:TrainedModel a rdfs:Class,
        owl:Class ;
    dct:contributor _:Ne8d6151e3d8047e6a947b3ec1a3830a1 ;
    dct:created "2024-12-01"^^xsd:date ;
    dct:source " 3.3.14"@en,
        "ISO/IEC 22989:2022"@en ;
    rdfs:isDefinedBy ai-owl: ;
    rdfs:subClassOf ai-owl:Model ;
    sw:term_status "accepted"@en ;
    skos:definition "Model resulted from model training"@en ;
    skos:prefLabel "Trained Model"@en .

ai-owl:TrainingData a rdfs:Class,
        owl:Class ;
    dct:contributor _:Ne8d6151e3d8047e6a947b3ec1a3830a1 ;
    dct:created "2024-12-01"^^xsd:date ;
    rdfs:isDefinedBy ai-owl: ;
    rdfs:subClassOf ai-owl:Data ;
    sw:term_status "accepted"@en ;
    skos:definition "Data involved in the training of an AI system or model"@en ;
    skos:prefLabel "Training Data"@en .

ai-owl:UnsupervisedLearning a rdfs:Class,
        owl:Class,
        ai-owl:Technique ;
    dct:contributor _:Ne8d6151e3d8047e6a947b3ec1a3830a1 ;
    dct:created "2024-12-01"^^xsd:date ;
    dct:source " 3.3.17"@en,
        "ISO/IEC 22989:2022"@en ;
    rdfs:isDefinedBy ai-owl: ;
    rdfs:subClassOf ai-owl:MachineLearning ;
    sw:term_status "accepted"@en ;
    skos:definition "Machine learning that makes only use of unlabelled data during training"@en ;
    skos:prefLabel "Unsupervised Learning"@en .

ai-owl:UpdateStage a rdfs:Class,
        owl:Class,
        ai-owl:LifecycleStage ;
    dct:contributor _:N0a43dd9ea5e94fe695d8b7df8802cfdd ;
    dct:created "2024-12-01"^^xsd:date ;
    dct:source "ISO/IEC 22989:2031"@en ;
    rdfs:isDefinedBy ai-owl: ;
    rdfs:subClassOf ai-owl:OperationStage ;
    sw:term_status "accepted"@en ;
    skos:definition "The stage in the lifecycle where an AI system is being or has been updated"@en ;
    skos:prefLabel "Update Stage"@en .

ai-owl:UserRisk a rdfs:Class,
        owl:Class,
        dpv-owl:RiskConcept,
        risk-owl:PotentialRisk,
        risk-owl:PotentialRiskSource ;
    dct:contributor _:Ne8d6151e3d8047e6a947b3ec1a3830a1 ;
    dct:created "2024-12-01"^^xsd:date ;
    rdfs:isDefinedBy ai-owl: ;
    rdfs:subClassOf ai-owl:RiskConcept ;
    sw:term_status "accepted"@en ;
    skos:definition "Risks associated with Users of AI Systems"@en ;
    skos:prefLabel "User Risk"@en .

ai-owl:ValidationData a rdfs:Class,
        owl:Class ;
    dct:contributor _:Ne8d6151e3d8047e6a947b3ec1a3830a1 ;
    dct:created "2024-12-01"^^xsd:date ;
    rdfs:isDefinedBy ai-owl: ;
    rdfs:subClassOf ai-owl:Data ;
    sw:term_status "accepted"@en ;
    skos:definition "Data involved in the validation of an AI system or model"@en ;
    skos:prefLabel "Validation Data"@en .

ai-owl:ValidationDataBias a rdfs:Class,
        owl:Class,
        dpv-owl:RiskConcept,
        risk-owl:PotentialRisk,
        risk-owl:PotentialRiskSource ;
    dct:contributor _:Ne8d6151e3d8047e6a947b3ec1a3830a1 ;
    dct:created "2024-12-01"^^xsd:date ;
    rdfs:isDefinedBy ai-owl: ;
    rdfs:subClassOf ai-owl:ValidationDataRisk ;
    sw:term_status "accepted"@en ;
    skos:definition "Concept representing validation data containing or potentially containing bias"@en ;
    skos:prefLabel "Validation Data Bias"@en .

ai-owl:ValidationDataInaccurate a rdfs:Class,
        owl:Class,
        dpv-owl:RiskConcept,
        risk-owl:PotentialRisk,
        risk-owl:PotentialRiskSource ;
    dct:contributor _:Ne8d6151e3d8047e6a947b3ec1a3830a1 ;
    dct:created "2024-12-01"^^xsd:date ;
    rdfs:isDefinedBy ai-owl: ;
    rdfs:subClassOf ai-owl:ValidationDataRisk ;
    sw:term_status "accepted"@en ;
    skos:definition "Concept representing validation data being inaccurate"@en ;
    skos:prefLabel "Validation Data Inaccurate"@en .

ai-owl:ValidationDataInappropriate a rdfs:Class,
        owl:Class,
        dpv-owl:RiskConcept,
        risk-owl:PotentialRisk,
        risk-owl:PotentialRiskSource ;
    dct:contributor _:Ne8d6151e3d8047e6a947b3ec1a3830a1 ;
    dct:created "2024-12-01"^^xsd:date ;
    rdfs:isDefinedBy ai-owl: ;
    rdfs:subClassOf ai-owl:ValidationDataRisk ;
    sw:term_status "accepted"@en ;
    skos:definition "Concept representing validation data being inappropriate"@en ;
    skos:prefLabel "Validation Data Inappropriate"@en .

ai-owl:ValidationDataIncomplete a rdfs:Class,
        owl:Class,
        dpv-owl:RiskConcept,
        risk-owl:PotentialRisk,
        risk-owl:PotentialRiskSource ;
    dct:contributor _:Ne8d6151e3d8047e6a947b3ec1a3830a1 ;
    dct:created "2024-12-01"^^xsd:date ;
    rdfs:isDefinedBy ai-owl: ;
    rdfs:subClassOf ai-owl:ValidationDataRisk ;
    sw:term_status "accepted"@en ;
    skos:definition "Concept representing validation data being incomplete"@en ;
    skos:prefLabel "Validation Data Incomplete"@en .

ai-owl:ValidationDataInconsistent a rdfs:Class,
        owl:Class,
        dpv-owl:RiskConcept,
        risk-owl:PotentialRisk,
        risk-owl:PotentialRiskSource ;
    dct:contributor _:Ne8d6151e3d8047e6a947b3ec1a3830a1 ;
    dct:created "2024-12-01"^^xsd:date ;
    rdfs:isDefinedBy ai-owl: ;
    rdfs:subClassOf ai-owl:ValidationDataRisk ;
    sw:term_status "accepted"@en ;
    skos:definition "Concept representing validation data being inconsistent"@en ;
    skos:prefLabel "Validation Data Inconsistent"@en .

ai-owl:ValidationDataMisclassified a rdfs:Class,
        owl:Class,
        dpv-owl:RiskConcept,
        risk-owl:PotentialRisk,
        risk-owl:PotentialRiskSource ;
    dct:contributor _:Ne8d6151e3d8047e6a947b3ec1a3830a1 ;
    dct:created "2024-12-01"^^xsd:date ;
    rdfs:isDefinedBy ai-owl: ;
    rdfs:subClassOf ai-owl:ValidationDataRisk ;
    sw:term_status "accepted"@en ;
    skos:definition "Concept representing validation data being misclassified"@en ;
    skos:prefLabel "Validation Data Misclassified"@en .

ai-owl:ValidationDataMisinterpretation a rdfs:Class,
        owl:Class,
        dpv-owl:RiskConcept,
        risk-owl:PotentialRisk,
        risk-owl:PotentialRiskSource ;
    dct:contributor _:Ne8d6151e3d8047e6a947b3ec1a3830a1 ;
    dct:created "2024-12-01"^^xsd:date ;
    rdfs:isDefinedBy ai-owl: ;
    rdfs:subClassOf ai-owl:ValidationDataRisk ;
    sw:term_status "accepted"@en ;
    skos:definition "Concept representing validation data being misinterpretation"@en ;
    skos:prefLabel "Validation Data Misinterpretation"@en .

ai-owl:ValidationDataNoise a rdfs:Class,
        owl:Class,
        dpv-owl:RiskConcept,
        risk-owl:PotentialRisk,
        risk-owl:PotentialRiskSource ;
    dct:contributor _:Ne8d6151e3d8047e6a947b3ec1a3830a1 ;
    dct:created "2024-12-01"^^xsd:date ;
    rdfs:isDefinedBy ai-owl: ;
    rdfs:subClassOf ai-owl:ValidationDataRisk ;
    sw:term_status "accepted"@en ;
    skos:definition "Concept representing validation data being noise"@en ;
    skos:prefLabel "Validation Data Noise"@en .

ai-owl:ValidationDataOutdated a rdfs:Class,
        owl:Class,
        dpv-owl:RiskConcept,
        risk-owl:PotentialRisk,
        risk-owl:PotentialRiskSource ;
    dct:contributor _:Ne8d6151e3d8047e6a947b3ec1a3830a1 ;
    dct:created "2024-12-01"^^xsd:date ;
    rdfs:isDefinedBy ai-owl: ;
    rdfs:subClassOf ai-owl:ValidationDataRisk ;
    sw:term_status "accepted"@en ;
    skos:definition "Concept representing validation data being outdated"@en ;
    skos:prefLabel "Validation Data Outdated"@en .

ai-owl:ValidationDataRisk a rdfs:Class,
        owl:Class,
        dpv-owl:RiskConcept,
        risk-owl:PotentialRisk,
        risk-owl:PotentialRiskSource ;
    dct:contributor _:Ne8d6151e3d8047e6a947b3ec1a3830a1 ;
    dct:created "2024-12-01"^^xsd:date ;
    rdfs:isDefinedBy ai-owl: ;
    rdfs:subClassOf ai-owl:DataRisk ;
    sw:term_status "accepted"@en ;
    skos:definition "Risks and risk concepts related to validation data"@en ;
    skos:prefLabel "Validation Data Risk"@en .

ai-owl:ValidationDataSelectionError a rdfs:Class,
        owl:Class,
        dpv-owl:RiskConcept,
        risk-owl:PotentialRisk,
        risk-owl:PotentialRiskSource ;
    dct:contributor _:Ne8d6151e3d8047e6a947b3ec1a3830a1 ;
    dct:created "2024-12-01"^^xsd:date ;
    rdfs:isDefinedBy ai-owl: ;
    rdfs:subClassOf ai-owl:ValidationDataRisk ;
    sw:term_status "accepted"@en ;
    skos:definition "Concept representing an error in validation data selection"@en ;
    skos:prefLabel "Validation Data Selection Error"@en .

ai-owl:ValidationDataSparse a rdfs:Class,
        owl:Class,
        dpv-owl:RiskConcept,
        risk-owl:PotentialRisk,
        risk-owl:PotentialRiskSource ;
    dct:contributor _:Ne8d6151e3d8047e6a947b3ec1a3830a1 ;
    dct:created "2024-12-01"^^xsd:date ;
    rdfs:isDefinedBy ai-owl: ;
    rdfs:subClassOf ai-owl:ValidationDataRisk ;
    sw:term_status "accepted"@en ;
    skos:definition "Concept representing validation data being sparse"@en ;
    skos:prefLabel "Validation Data Sparse"@en .

ai-owl:ValidationDataUnrepresentative a rdfs:Class,
        owl:Class,
        dpv-owl:RiskConcept,
        risk-owl:PotentialRisk,
        risk-owl:PotentialRiskSource ;
    dct:contributor _:Ne8d6151e3d8047e6a947b3ec1a3830a1 ;
    dct:created "2024-12-01"^^xsd:date ;
    rdfs:isDefinedBy ai-owl: ;
    rdfs:subClassOf ai-owl:ValidationDataRisk ;
    sw:term_status "accepted"@en ;
    skos:definition "Concept representing validation data being unrepresentative"@en ;
    skos:prefLabel "Validation Data Unrepresentative"@en .

ai-owl:ValidationDataUnstructured a rdfs:Class,
        owl:Class,
        dpv-owl:RiskConcept,
        risk-owl:PotentialRisk,
        risk-owl:PotentialRiskSource ;
    dct:contributor _:Ne8d6151e3d8047e6a947b3ec1a3830a1 ;
    dct:created "2024-12-01"^^xsd:date ;
    rdfs:isDefinedBy ai-owl: ;
    rdfs:subClassOf ai-owl:ValidationDataRisk ;
    sw:term_status "accepted"@en ;
    skos:definition "Concept representing validation data being unstructured"@en ;
    skos:prefLabel "Validation Data Unstructured"@en .

ai-owl:ValidationDataUnverified a rdfs:Class,
        owl:Class,
        dpv-owl:RiskConcept,
        risk-owl:PotentialRisk,
        risk-owl:PotentialRiskSource ;
    dct:contributor _:Ne8d6151e3d8047e6a947b3ec1a3830a1 ;
    dct:created "2024-12-01"^^xsd:date ;
    rdfs:isDefinedBy ai-owl: ;
    rdfs:subClassOf ai-owl:ValidationDataRisk ;
    sw:term_status "accepted"@en ;
    skos:definition "Concept representing validation data being unverified"@en ;
    skos:prefLabel "Validation Data Unverified"@en .

ai-owl:ValidationStage a rdfs:Class,
        owl:Class,
        ai-owl:LifecycleStage ;
    dct:contributor _:Ne8d6151e3d8047e6a947b3ec1a3830a1 ;
    dct:created "2024-12-01"^^xsd:date ;
    dct:source "ISO/IEC 22989:2026"@en ;
    rdfs:isDefinedBy ai-owl: ;
    rdfs:subClassOf ai-owl:LifecycleStage ;
    sw:term_status "accepted"@en ;
    skos:definition "The stage in the lifecycle where the AI system is validated for requirements and objectives for an intended use or application"@en ;
    skos:prefLabel "Validation Stage"@en .

ai-owl:VerificationStage a rdfs:Class,
        owl:Class,
        ai-owl:LifecycleStage ;
    dct:contributor _:Ne8d6151e3d8047e6a947b3ec1a3830a1 ;
    dct:created "2024-12-01"^^xsd:date ;
    dct:source "ISO/IEC 22989:2025"@en ;
    rdfs:isDefinedBy ai-owl: ;
    rdfs:subClassOf ai-owl:LifecycleStage ;
    sw:term_status "accepted"@en ;
    skos:definition "The stage in the lifecycle where the AI system is being verified to satisfy requirements and meet objectives"@en ;
    skos:prefLabel "Verification Stage"@en .

ai-owl:VideoGeneration a rdfs:Class,
        owl:Class,
        ai-owl:Capability ;
    dct:contributor _:N0a43dd9ea5e94fe695d8b7df8802cfdd,
        _:Ne8d6151e3d8047e6a947b3ec1a3830a1 ;
    dct:created "2024-12-01"^^xsd:date ;
    rdfs:isDefinedBy ai-owl: ;
    rdfs:subClassOf ai-owl:ContentGeneration ;
    sw:term_status "accepted"@en ;
    skos:definition "Capability to generate video"@en ;
    skos:prefLabel "Video Generation"@en .

ai-owl:hasAISystem a rdf:Property,
        owl:ObjectProperty ;
    dcam:rangeIncludes ai-owl:AISystem ;
    dct:contributor _:Ne8d6151e3d8047e6a947b3ec1a3830a1 ;
    dct:created "2024-12-01"^^xsd:date ;
    rdfs:isDefinedBy ai-owl: ;
    rdfs:subPropertyOf ai-owl:hasAI ;
    sw:term_status "accepted"@en ;
    skos:definition "Indicates the use of AI system for the associated context"@en ;
    skos:prefLabel "has AI system"@en ;
    schema:rangeIncludes ai-owl:AISystem .

ai-owl:hasCapability a rdf:Property,
        owl:ObjectProperty ;
    dcam:rangeIncludes ai-owl:Capability ;
    dct:contributor _:Ne8d6151e3d8047e6a947b3ec1a3830a1 ;
    dct:created "2024-12-01"^^xsd:date ;
    rdfs:isDefinedBy ai-owl: ;
    rdfs:subPropertyOf ai-owl:hasAI ;
    sw:term_status "accepted"@en ;
    skos:definition "Indicates the use of AI capability for the associated context"@en ;
    skos:prefLabel "has capability"@en ;
    schema:rangeIncludes ai-owl:Capability .

ai-owl:hasGPAIModel a rdf:Property,
        owl:ObjectProperty ;
    dcam:rangeIncludes ai-owl:GPAIModel ;
    dct:contributor _:Ne8d6151e3d8047e6a947b3ec1a3830a1 ;
    dct:created "2024-12-01"^^xsd:date ;
    rdfs:isDefinedBy ai-owl: ;
    rdfs:subPropertyOf ai-owl:hasModel ;
    sw:term_status "accepted"@en ;
    skos:definition "Indicates the use of an GPAI model for the associated context"@en ;
    skos:prefLabel "has GPAI model"@en ;
    schema:rangeIncludes ai-owl:GPAIModel .

ai-owl:hasTechnique a rdf:Property,
        owl:ObjectProperty ;
    dcam:rangeIncludes ai-owl:Technique ;
    dct:contributor _:Ne8d6151e3d8047e6a947b3ec1a3830a1 ;
    dct:created "2024-12-01"^^xsd:date ;
    rdfs:isDefinedBy ai-owl: ;
    rdfs:subPropertyOf ai-owl:hasAI ;
    sw:term_status "accepted"@en ;
    skos:definition "Indicates the use of AI technique for the associated context"@en ;
    skos:prefLabel "has technique"@en ;
    schema:rangeIncludes ai-owl:Technique .

ai-owl:hasTestingData a rdf:Property,
        owl:ObjectProperty ;
    dcam:domainIncludes ai-owl:AI ;
    dcam:rangeIncludes ai-owl:ValidationData ;
    dct:contributor _:Ne8d6151e3d8047e6a947b3ec1a3830a1 ;
    dct:created "2024-12-01"^^xsd:date ;
    rdfs:isDefinedBy ai-owl: ;
    rdfs:subPropertyOf ai-owl:hasData,
        tech-owl:hasInputData ;
    sw:term_status "accepted"@en ;
    skos:definition "Associates the data used for testing AI"@en ;
    skos:prefLabel "has testing data"@en ;
    schema:domainIncludes ai-owl:AI ;
    schema:rangeIncludes ai-owl:ValidationData .

ai-owl:hasTrainingData a rdf:Property,
        owl:ObjectProperty ;
    dcam:domainIncludes ai-owl:AI ;
    dcam:rangeIncludes ai-owl:TestingData ;
    dct:contributor _:Ne8d6151e3d8047e6a947b3ec1a3830a1 ;
    dct:created "2024-12-01"^^xsd:date ;
    rdfs:isDefinedBy ai-owl: ;
    rdfs:subPropertyOf ai-owl:hasData,
        tech-owl:hasInputData ;
    sw:term_status "accepted"@en ;
    skos:definition "Associates the data used for training AI"@en ;
    skos:prefLabel "has training data"@en ;
    schema:domainIncludes ai-owl:AI ;
    schema:rangeIncludes ai-owl:TestingData .

ai-owl:hasValidationData a rdf:Property,
        owl:ObjectProperty ;
    dcam:domainIncludes ai-owl:AI ;
    dcam:rangeIncludes ai-owl:TrainingData ;
    dct:contributor _:Ne8d6151e3d8047e6a947b3ec1a3830a1 ;
    dct:created "2024-12-01"^^xsd:date ;
    rdfs:isDefinedBy ai-owl: ;
    rdfs:subPropertyOf ai-owl:hasData,
        tech-owl:hasInputData ;
    sw:term_status "accepted"@en ;
    skos:definition "Associates the data used for validating AI"@en ;
    skos:prefLabel "has validation data"@en ;
    schema:domainIncludes ai-owl:AI ;
    schema:rangeIncludes ai-owl:TrainingData .

ai-owl:hasModel a rdf:Property,
        owl:ObjectProperty ;
    dcam:rangeIncludes ai-owl:Model ;
    dct:contributor _:Ne8d6151e3d8047e6a947b3ec1a3830a1 ;
    dct:created "2024-12-01"^^xsd:date ;
    rdfs:isDefinedBy ai-owl: ;
    rdfs:subPropertyOf ai-owl:hasAI ;
    sw:term_status "accepted"@en ;
    skos:definition "Indicates the use of an AI model for the associated context"@en ;
    skos:prefLabel "has model"@en ;
    schema:rangeIncludes ai-owl:Model .

ai-owl:serialisation-html a profile:ResourceDescriptor ;
    dct:conformsTo <https://www.w3.org/TR/html/> ;
    dct:format <https://www.iana.org/assignments/media-types/text/html> ;
    dct:title "AI Technology Concepts - HTML serialiation" ;
    profile:hasArtifact <https://w3id.org/dpv/ai/ai-owl.html> ;
    profile:hasRole role:specification .

ai-owl:serialisation-jsonld a profile:ResourceDescriptor ;
    dct:conformsTo <https://www.w3.org/TR/json-ld11/> ;
    dct:format <https://www.iana.org/assignments/media-types/application/ld+json> ;
    dct:title "AI Technology Concepts - JSON-LD serialiation" ;
    profile:hasArtifact <https://w3id.org/dpv/ai/ai-owl.jsonld> ;
    profile:hasRole role:vocabulary .

ai-owl:serialisation-n3 a profile:ResourceDescriptor ;
    dct:conformsTo <https://www.w3.org/TeamSubmission/n3/> ;
    dct:format <https://www.iana.org/assignments/media-types/text/n3> ;
    dct:title "AI Technology Concepts - N3 serialiation" ;
    profile:hasArtifact <https://w3id.org/dpv/ai/ai-owl.n3> ;
    profile:hasRole role:vocabulary .

ai-owl:serialisation-rdf a profile:ResourceDescriptor ;
    dct:conformsTo rdf: ;
    dct:format <https://www.iana.org/assignments/media-types/application/rdf+xml> ;
    dct:title "AI Technology Concepts - RDF/XML serialiation" ;
    profile:hasArtifact <https://w3id.org/dpv/ai/ai-owl.rdf> ;
    profile:hasRole role:vocabulary .

ai-owl:serialisation-ttl a profile:ResourceDescriptor ;
    dct:conformsTo <https://www.w3.org/TR/turtle/> ;
    dct:format <https://www.iana.org/assignments/media-types/text/turtle> ;
    dct:title "AI Technology Concepts - Turtle serialiation" ;
    profile:hasArtifact <https://w3id.org/dpv/ai/ai-owl.ttl> ;
    profile:hasRole role:vocabulary .

<https://w3id.org/dpv/examples> a profile:ResourceDescriptor ;
    dct:conformsTo <https://www.w3.org/TR/html/> ;
    dct:format <https://www.iana.org/assignments/media-types/text/html> ;
    dct:title "Examples for Data Privacy Vocabulary" ;
    profile:hasArtifact <https://w3id.org/dpv/examples> ;
    profile:hasRole role:guidance .

<https://w3id.org/dpv/guides> a profile:ResourceDescriptor ;
    dct:conformsTo <https://www.w3.org/TR/html/> ;
    dct:format <https://www.iana.org/assignments/media-types/text/html> ;
    dct:title "Guides for Data Privacy Vocabulary" ;
    profile:hasArtifact <https://w3id.org/dpv/guides> ;
    profile:hasRole role:guidance .

<https://w3id.org/dpv/primer> a profile:ResourceDescriptor ;
    dct:conformsTo <https://www.w3.org/TR/html/> ;
    dct:format <https://www.iana.org/assignments/media-types/text/html> ;
    dct:title "Primer for Data Privacy Vocabulary" ;
    profile:hasArtifact <https://w3id.org/dpv/primer> ;
    profile:hasRole role:guidance .

ai-owl:hasData a rdf:Property,
        owl:ObjectProperty ;
    dcam:domainIncludes ai-owl:AI ;
    dcam:rangeIncludes ai-owl:Data ;
    dct:contributor _:N0a43dd9ea5e94fe695d8b7df8802cfdd ;
    dct:created "2024-12-01"^^xsd:date ;
    rdfs:isDefinedBy ai-owl: ;
    rdfs:subPropertyOf dpv-owl:hasData ;
    sw:term_status "accepted"@en ;
    skos:definition "Associates data with an AI system or model or implementation"@en ;
    skos:prefLabel "has data"@en ;
    schema:domainIncludes ai-owl:AI ;
    schema:rangeIncludes ai-owl:Data .

ai-owl:hasAI a rdf:Property,
        owl:ObjectProperty ;
    dcam:rangeIncludes ai-owl:AI ;
    dct:contributor _:Ne8d6151e3d8047e6a947b3ec1a3830a1 ;
    dct:created "2024-12-01"^^xsd:date ;
    rdfs:isDefinedBy ai-owl: ;
    rdfs:subPropertyOf dpv-owl:isImplementedUsingTechnology ;
    sw:term_status "accepted"@en ;
    skos:definition "Indicates the use of AI for the associated context"@en ;
    skos:prefLabel "has AI"@en ;
    schema:rangeIncludes ai-owl:AI .

ai-owl: a owl:Ontology,
        profile:Profile ;
    dct:bibliographicCitation "Harshvardhan J. Pandit, Beatriz Esteves, Georg P. Krog, Paul Ryan, Delaram Golpayegani, Julian Flake (2025) Data Privacy Vocabulary (DPV) – Version 2.0. In: Demartini, G., et al. The Semantic Web – ISWC 2024. ISWC 2024. Lecture Notes in Computer Science, vol 15233. Springer, Cham. https://doi.org/10.1007/978-3-031-77847-6_10" ;
    dct:conformsTo <http://www.w3.org/2002/07/owl>,
        "http://www.w3.org/2000/01/rdf-schema",
        "http://www.w3.org/2004/02/skos/core" ;
    dct:contributor _:N0a43dd9ea5e94fe695d8b7df8802cfdd,
        _:N606ea170c32e4fb5ac26e62242d8681b,
        _:Ne8d6151e3d8047e6a947b3ec1a3830a1 ;
    dct:created "2024-05-31"@en ;
    dct:creator _:N0a43dd9ea5e94fe695d8b7df8802cfdd,
        _:Ne8d6151e3d8047e6a947b3ec1a3830a1 ;
    dct:description "Extension to the Data Privacy Vocabulary (DPV) providing concepts for representing information about AI technologies"@en ;
    dct:hasVersion ai-owl: ;
    dct:identifier "https://w3id.org/dpv/ai" ;
    dct:issued "2024-05-31"@en ;
    dct:license <https://www.w3.org/copyright/document-license-2023/> ;
    dct:modified "2025-03-16"@en ;
    dct:publisher <https://www.w3.org/> ;
    dct:source <https://www.w3.org/groups/cg/dpvcg/> ;
    dct:title "AI Technology Concepts"@en ;
    bibo:doi "10.5281/zenodo.12505841" ;
    bibo:status "http://purl.org/ontology/bibo/status/published" ;
    vann:preferredNamespacePrefix "ai" ;
    vann:preferredNamespaceUri "https://w3id.org/dpv/ai#" ;
    rdfs:Label "AI"@en ;
    owl:versionIRI <https://w3id.org/dpv/2.1/ai/owl#> ;
    owl:versionInfo "2.1" ;
    profile:hasResource ai-owl:serialisation-html,
        ai-owl:serialisation-jsonld,
        ai-owl:serialisation-n3,
        ai-owl:serialisation-rdf,
        ai-owl:serialisation-ttl,
        <https://w3id.org/dpv/examples>,
        <https://w3id.org/dpv/guides>,
        <https://w3id.org/dpv/primer> ;
    profile:isProfileOf <http://www.w3.org/2002/07/owl>,
        ai-owl:,
        <https://w3id.org/dpv/tech/owl> ;
    foaf:logo <https://w3id.org/dpv/media/logo.png> ;
    schema:version "2.1" .

_:N088477eac8b34fdc990d41104955af14 a foaf:Organization ;
    foaf:name "Trinity College Dublin" .

_:N2107ae3007164122b8f508ef58f07bab a foaf:Organization ;
    foaf:name "ADAPT Centre, Trinity College Dublin" .

_:N313d89a6c37147bfac1bbb4aa7f6510b a foaf:Organization ;
    foaf:name "ADAPT Centre, Dublin City University" .

_:N606ea170c32e4fb5ac26e62242d8681b a dct:Agent,
        foaf:Person ;
    org:memberOf _:N088477eac8b34fdc990d41104955af14 ;
    foaf:name "Daniel Doherty" .

_:N0a43dd9ea5e94fe695d8b7df8802cfdd a dct:Agent,
        foaf:Person ;
    scoro:hasORCID "0000-0002-5068-3714" ;
    org:memberOf _:N313d89a6c37147bfac1bbb4aa7f6510b ;
    foaf:homepage "https://harshp.com/" ;
    foaf:name "Harshvardhan J. Pandit" .

_:Ne8d6151e3d8047e6a947b3ec1a3830a1 a dct:Agent,
        foaf:Person ;
    scoro:hasORCID "0000-0002-1208-186X" ;
    org:memberOf _:N2107ae3007164122b8f508ef58f07bab ;
    foaf:name "Delaram Golpayegani" .

