@prefix bibo: <http://purl.org/ontology/bibo/> .
@prefix dct: <http://purl.org/dc/terms/> .
@prefix dpv-owl: <https://w3id.org/dpv/owl#> .
@prefix foaf: <http://xmlns.com/foaf/0.1/> .
@prefix org: <http://www.w3.org/ns/org#> .
@prefix owl: <http://www.w3.org/2002/07/owl#> .
@prefix profile: <http://www.w3.org/ns/dx/prof/> .
@prefix rdf: <http://www.w3.org/1999/02/22-rdf-syntax-ns#> .
@prefix rdfs: <http://www.w3.org/2000/01/rdf-schema#> .
@prefix role: <http://www.w3.org/ns/dx/prof/role/> .
@prefix schema: <https://schema.org/> .
@prefix scoro: <http://purl.org/spar/scoro/> .
@prefix skos: <http://www.w3.org/2004/02/skos/core#> .
@prefix sw: <http://www.w3.org/2003/06/sw-vocab-status/ns#> .
@prefix vann: <http://purl.org/vocab/vann/> .
@prefix xsd: <http://www.w3.org/2001/XMLSchema#> .

dpv-owl:ConsentControl a rdfs:Class,
        owl:Class ;
    dct:created "2024-05-11"^^xsd:date ;
    rdfs:isDefinedBy dpv-owl: ;
    rdfs:subClassOf dpv-owl:EntityInvolvement ;
    sw:term_status "accepted"@en ;
    skos:definition "The control or activity associated with obtaining, providing, withdrawing, or reaffirming consent"@en ;
    skos:prefLabel "Consent Control"@en .

dpv-owl:ManageConsent a rdfs:Class,
        owl:Class ;
    dct:created "2024-12-17"^^xsd:date ;
    rdfs:isDefinedBy dpv-owl: ;
    rdfs:subClassOf dpv-owl:ProvideConsent,
        dpv-owl:ReaffirmConsent,
        dpv-owl:WithdrawConsent ;
    sw:term_status "accepted"@en ;
    skos:definition "Control for managing a given consent in terms of providing, reaffirming, or withdrawing it"@en ;
    skos:prefLabel "Manage Consent"@en ;
    skos:scopeNote "Indicates how the data subject can manage their consent in terms of providing it, or reaffirming or withdrawing a given consent. This concept is useful to represent a single location or interface where multiple controls are provided for consent"@en .

dpv-owl:ObtainConsent a rdfs:Class,
        owl:Class ;
    dct:created "2024-05-11"^^xsd:date ;
    rdfs:isDefinedBy dpv-owl: ;
    rdfs:subClassOf dpv-owl:ConsentControl ;
    sw:term_status "accepted"@en ;
    skos:definition "Control for obtaining consent"@en ;
    skos:prefLabel "Obtain Consent"@en ;
    skos:scopeNote "Indicates how the controller or entity can obtain consent e.g. used with dpv:isExercisedAt"@en .

dpv-owl:ProvideConsent a rdfs:Class,
        owl:Class ;
    dct:created "2024-05-11"^^xsd:date ;
    rdfs:isDefinedBy dpv-owl: ;
    rdfs:subClassOf dpv-owl:ConsentControl,
        dpv-owl:OptingInToProcess ;
    sw:term_status "accepted"@en ;
    skos:definition "Control for providing consent"@en ;
    skos:prefLabel "Provide Consent"@en ;
    skos:scopeNote "Indicates how the data subject can provide consent e.g. used with dpv:isExercisedAt"@en .

dpv-owl:ReaffirmConsent a rdfs:Class,
        owl:Class ;
    dct:created "2024-05-11"^^xsd:date ;
    rdfs:isDefinedBy dpv-owl: ;
    rdfs:subClassOf dpv-owl:ConsentControl ;
    sw:term_status "accepted"@en ;
    skos:definition "Control for affirming consent"@en ;
    skos:prefLabel "Reaffirm Consent"@en ;
    skos:scopeNote "Indicates how the controller (with dpv:ObtainConsent) or data subject (with dpv:ProvideConsent) can reaffirm consent e.g. used with dpv:isExercisedAt"@en .

dpv-owl:RefuseConsent a rdfs:Class,
        owl:Class ;
    dct:created "2024-12-17"^^xsd:date ;
    rdfs:isDefinedBy dpv-owl: ;
    rdfs:subClassOf dpv-owl:ConsentControl ;
    sw:term_status "accepted"@en ;
    skos:definition "Control for refusing consent"@en ;
    skos:prefLabel "Refuse Consent"@en ;
    skos:scopeNote "Indicates how the controller (with dpv:ObtainConsent) or data subject (with dpv:ProvideConsent) can reaffirm consent e.g. used with dpv:isExercisedAt"@en .

dpv-owl:WithdrawConsent a rdfs:Class,
        owl:Class ;
    dct:created "2024-05-11"^^xsd:date ;
    rdfs:isDefinedBy dpv-owl: ;
    rdfs:subClassOf dpv-owl:ConsentControl,
        dpv-owl:WithdrawingFromProcess ;
    sw:term_status "accepted"@en ;
    skos:definition "Control for withdrawing consent"@en ;
    skos:prefLabel "Withdraw Consent"@en ;
    skos:scopeNote "Indicates how the data subject can withdraw consent e.g. used with dpv:isExercisedAt"@en .

dpv-owl:serialisation-html a profile:ResourceDescriptor ;
    dct:conformsTo <https://www.w3.org/TR/html/> ;
    dct:format <https://www.iana.org/assignments/media-types/text/html> ;
    dct:title "Data Privacy Vocabulary (DPV) - HTML serialiation" ;
    profile:hasArtifact <https://w3id.org/dpv/dpv-owl.html> ;
    profile:hasRole role:specification .

dpv-owl:serialisation-jsonld a profile:ResourceDescriptor ;
    dct:conformsTo <https://www.w3.org/TR/json-ld11/> ;
    dct:format <https://www.iana.org/assignments/media-types/application/ld+json> ;
    dct:title "Data Privacy Vocabulary (DPV) - JSON-LD serialiation" ;
    profile:hasArtifact <https://w3id.org/dpv/dpv/dpv-owl.jsonld> ;
    profile:hasRole role:vocabulary .

dpv-owl:serialisation-n3 a profile:ResourceDescriptor ;
    dct:conformsTo <https://www.w3.org/TeamSubmission/n3/> ;
    dct:format <https://www.iana.org/assignments/media-types/text/n3> ;
    dct:title "Data Privacy Vocabulary (DPV) - N3 serialiation" ;
    profile:hasArtifact <https://w3id.org/dpv/dpv/dpv-owl.n3> ;
    profile:hasRole role:vocabulary .

dpv-owl:serialisation-rdf a profile:ResourceDescriptor ;
    dct:conformsTo rdf: ;
    dct:format <https://www.iana.org/assignments/media-types/application/rdf+xml> ;
    dct:title "Data Privacy Vocabulary (DPV) - RDF/XML serialiation" ;
    profile:hasArtifact <https://w3id.org/dpv/dpv/dpv-owl.rdf> ;
    profile:hasRole role:vocabulary .

dpv-owl:serialisation-ttl a profile:ResourceDescriptor ;
    dct:conformsTo <https://www.w3.org/TR/turtle/> ;
    dct:format <https://www.iana.org/assignments/media-types/text/turtle> ;
    dct:title "Data Privacy Vocabulary (DPV) - Turtle serialiation" ;
    profile:hasArtifact <https://w3id.org/dpv/dpv/dpv-owl.ttl> ;
    profile:hasRole role:vocabulary .

<https://w3id.org/dpv/examples> a profile:ResourceDescriptor ;
    dct:conformsTo <https://www.w3.org/TR/html/> ;
    dct:format <https://www.iana.org/assignments/media-types/text/html> ;
    dct:title "Examples for Data Privacy Vocabulary" ;
    profile:hasArtifact <https://w3id.org/dpv/examples> ;
    profile:hasRole role:guidance .

<https://w3id.org/dpv/guides> a profile:ResourceDescriptor ;
    dct:conformsTo <https://www.w3.org/TR/html/> ;
    dct:format <https://www.iana.org/assignments/media-types/text/html> ;
    dct:title "Guides for Data Privacy Vocabulary" ;
    profile:hasArtifact <https://w3id.org/dpv/guides> ;
    profile:hasRole role:guidance .

<https://w3id.org/dpv/primer> a profile:ResourceDescriptor ;
    dct:conformsTo <https://www.w3.org/TR/html/> ;
    dct:format <https://www.iana.org/assignments/media-types/text/html> ;
    dct:title "Primer for Data Privacy Vocabulary" ;
    profile:hasArtifact <https://w3id.org/dpv/primer> ;
    profile:hasRole role:guidance .

dpv-owl: a owl:Ontology,
        profile:Profile ;
    dct:bibliographicCitation "Harshvardhan J. Pandit, Beatriz Esteves, Georg P. Krog, Paul Ryan, Delaram Golpayegani, Julian Flake (2025) Data Privacy Vocabulary (DPV) – Version 2.0. In: Demartini, G., et al. The Semantic Web – ISWC 2024. ISWC 2024. Lecture Notes in Computer Science, vol 15233. Springer, Cham. https://doi.org/10.1007/978-3-031-77847-6_10" ;
    dct:conformsTo <http://www.w3.org/2002/07/owl>,
        "http://www.w3.org/2000/01/rdf-schema",
        "http://www.w3.org/2004/02/skos/core" ;
    dct:created "2022-08-18"@en ;
    dct:creator [ a dct:Agent,
                foaf:Person ;
            org:memberOf [ a foaf:Organization ;
                    foaf:name "Signatu AS" ] ;
            foaf:homepage "https://www.linkedin.com/in/georg-philip-krog-a2a278104/" ;
            foaf:name "Georg P. Krog" ],
        [ a dct:Agent,
                foaf:Person ;
            scoro:hasORCID "0000-0002-5068-3714" ;
            org:memberOf [ a foaf:Organization ;
                    foaf:name "ADAPT Centre, Dublin City University" ] ;
            foaf:homepage "https://harshp.com/" ;
            foaf:name "Harshvardhan J. Pandit" ],
        [ a dct:Agent,
                foaf:Person ;
            scoro:hasORCID "0009-0006-4623-1463" ;
            org:memberOf [ a foaf:Organization ;
                    foaf:name "University of Koblenz" ] ;
            foaf:name "Julian Flake" ],
        [ a dct:Agent,
                foaf:Person ;
            scoro:hasORCID "0000-0003-0259-7560" ;
            org:memberOf [ a foaf:Organization ;
                    foaf:name "IDLab, IMEC, Ghent University" ] ;
            foaf:name "Beatriz Esteves" ],
        [ a dct:Agent,
                foaf:Person ;
            scoro:hasORCID "0000-0003-0770-2737" ;
            org:memberOf [ a foaf:Organization ;
                    foaf:name "Uniphar PLC" ] ;
            foaf:name "Paul Ryan" ],
        [ a dct:Agent,
                foaf:Person ;
            scoro:hasORCID "0000-0002-1208-186X" ;
            org:memberOf [ a foaf:Organization ;
                    foaf:name "ADAPT Centre, Trinity College Dublin" ] ;
            foaf:name "Delaram Golpayegani" ] ;
    dct:description "The Data Privacy Vocabulary (DPV) provides terms (classes and properties) to represent information about processing of personal data, for example - purposes, processing operations, personal data, technical and organisational measures."@en ;
    dct:hasVersion dpv-owl: ;
    dct:identifier "https://w3id.org/dpv" ;
    dct:issued "2022-08-18"@en ;
    dct:license <https://www.w3.org/copyright/document-license-2023/> ;
    dct:modified "2025-03-16"@en ;
    dct:publisher <https://www.w3.org/> ;
    dct:source <https://www.w3.org/groups/cg/dpvcg/> ;
    dct:title "Data Privacy Vocabulary (DPV)"@en ;
    bibo:doi "10.5281/zenodo.12505841" ;
    bibo:status "http://purl.org/ontology/bibo/status/published" ;
    vann:preferredNamespacePrefix "dpv" ;
    vann:preferredNamespaceUri "https://w3id.org/dpv#" ;
    rdfs:Label "DPV"@en ;
    owl:versionIRI <https://w3id.org/dpv/2.1/owl#> ;
    owl:versionInfo "2.1" ;
    profile:hasResource <https://w3id.org/dpv/examples>,
        <https://w3id.org/dpv/guides>,
        dpv-owl:serialisation-html,
        dpv-owl:serialisation-jsonld,
        dpv-owl:serialisation-n3,
        dpv-owl:serialisation-rdf,
        dpv-owl:serialisation-ttl,
        <https://w3id.org/dpv/primer> ;
    profile:isProfileOf <http://www.w3.org/2002/07/owl>,
        dpv-owl: ;
    foaf:logo <https://w3id.org/dpv/media/logo.png> ;
    schema:version "2.1" .

