@prefix bibo: <http://purl.org/ontology/bibo/> .
@prefix dct: <http://purl.org/dc/terms/> .
@prefix dex-owl: <https://w3id.org/dpv/examples/owl#> .
@prefix dpv-owl: <https://w3id.org/dpv/owl#> .
@prefix foaf: <http://xmlns.com/foaf/0.1/> .
@prefix org: <http://www.w3.org/ns/org#> .
@prefix owl: <http://www.w3.org/2002/07/owl#> .
@prefix profile: <http://www.w3.org/ns/dx/prof/> .
@prefix rdf: <http://www.w3.org/1999/02/22-rdf-syntax-ns#> .
@prefix rdfs: <http://www.w3.org/2000/01/rdf-schema#> .
@prefix role: <http://www.w3.org/ns/dx/prof/role/> .
@prefix schema: <https://schema.org/> .
@prefix scoro: <http://purl.org/spar/scoro/> .
@prefix skos: <http://www.w3.org/2004/02/skos/core#> .
@prefix sw: <http://www.w3.org/2003/06/sw-vocab-status/ns#> .
@prefix vann: <http://purl.org/vocab/vann/> .
@prefix xsd: <http://www.w3.org/2001/XMLSchema#> .

dpv-owl:ContractAmendmentClause a rdfs:Class,
        owl:Class,
        dpv-owl:ContractualClause ;
    dct:created "2024-08-27"^^xsd:date ;
    rdfs:isDefinedBy dpv-owl: ;
    rdfs:subClassOf dpv-owl:ContractualClause ;
    sw:term_status "accepted"@en ;
    skos:definition "A provision describing how changes or modifications to the contract can be made and the process for implementing them"@en ;
    skos:prefLabel "Contract Amendment Clause"@en .

dpv-owl:ContractConfidentialityClause a rdfs:Class,
        owl:Class,
        dpv-owl:ContractualClause ;
    dct:created "2024-08-27"^^xsd:date ;
    rdfs:isDefinedBy dpv-owl: ;
    rdfs:subClassOf dpv-owl:ContractualClause ;
    sw:term_status "accepted"@en ;
    skos:definition "A provision requiring parties to keep certain information confidential and not disclose it to third parties"@en ;
    skos:prefLabel "Contract Confidentiality Clause"@en .

dpv-owl:ContractDefinitions a rdfs:Class,
        owl:Class,
        dpv-owl:ContractualClause ;
    dct:created "2024-08-27"^^xsd:date ;
    rdfs:isDefinedBy dpv-owl: ;
    rdfs:subClassOf dpv-owl:ContractualClause ;
    sw:term_status "accepted"@en ;
    skos:definition "A section specifying the meanings of key terms and phrases used throughout the contract"@en ;
    skos:prefLabel "Contract Definitions"@en .

dpv-owl:ContractDisputeResolutionClause a rdfs:Class,
        owl:Class,
        dpv-owl:ContractualClause ;
    dct:created "2024-08-27"^^xsd:date ;
    rdfs:isDefinedBy dpv-owl: ;
    rdfs:subClassOf dpv-owl:ContractualClause ;
    sw:term_status "accepted"@en ;
    skos:definition "A provision detailing the methods and procedures for resolving disagreements or conflicts arising from the contract"@en ;
    skos:prefLabel "Contract DisputeResolution Clause"@en .

dpv-owl:ContractJurisdictionClause a rdfs:Class,
        owl:Class,
        dpv-owl:ContractualClause ;
    dct:created "2024-08-27"^^xsd:date ;
    rdfs:isDefinedBy dpv-owl: ;
    rdfs:subClassOf dpv-owl:ContractualClause ;
    sw:term_status "accepted"@en ;
    skos:definition "A provision specifying the legal jurisdiction or court where disputes related to the contract will be resolved"@en ;
    skos:prefLabel "Contract Jurisdiction Clause"@en .

dpv-owl:ContractPreamble a rdfs:Class,
        owl:Class,
        dpv-owl:ContractualClause ;
    dct:created "2024-08-27"^^xsd:date ;
    rdfs:isDefinedBy dpv-owl: ;
    rdfs:subClassOf dpv-owl:ContractualClause ;
    sw:term_status "accepted"@en ;
    skos:definition "An introductory section outlining the background, context, and purpose of the contract"@en ;
    skos:prefLabel "Contract Preamble"@en .

dpv-owl:ContractTerminationClause a rdfs:Class,
        owl:Class,
        dpv-owl:ContractualClause ;
    dct:created "2024-08-27"^^xsd:date ;
    rdfs:isDefinedBy dpv-owl: ;
    rdfs:subClassOf dpv-owl:ContractualClause ;
    sw:term_status "accepted"@en ;
    skos:definition "A provision outlining the conditions under which the contract can be terminated before its completion, including any penalties or obligations"@en ;
    skos:prefLabel "Contract Termination Clause"@en .

dpv-owl:ContractualClause a rdfs:Class,
        owl:Class ;
    dct:created "2024-08-27"^^xsd:date ;
    vann:example dex-owl:E0078 ;
    rdfs:isDefinedBy dpv-owl: ;
    sw:term_status "accepted"@en ;
    skos:definition "A part or component within a contract that outlines its specifics"@en ;
    skos:prefLabel "Contractual Clause"@en .

dpv-owl:ContractualClauseFulfiled a rdfs:Class,
        owl:Class,
        dpv-owl:ContractualClauseFulfilmentStatus ;
    dct:created "2024-08-27"^^xsd:date ;
    rdfs:isDefinedBy dpv-owl: ;
    rdfs:subClassOf dpv-owl:ContractualClauseFulfilmentStatus ;
    sw:term_status "accepted"@en ;
    skos:definition "Status indicating the terms of the contractual clause are fulfiled i.e. they have been succesfully completed without violation"@en ;
    skos:prefLabel "Contractual Clause Fulfiled"@en .

dpv-owl:ContractualClauseFulfilmentStatus a rdfs:Class,
        owl:Class ;
    dct:created "2024-08-27"^^xsd:date ;
    rdfs:isDefinedBy dpv-owl: ;
    rdfs:subClassOf dpv-owl:ContractStatus ;
    sw:term_status "accepted"@en ;
    skos:definition "Status associated with fulfilment of a contractual clause"@en ;
    skos:prefLabel "Contractual Clause Fulfilment Status"@en .

dpv-owl:ContractualClauseNotFulfiled a rdfs:Class,
        owl:Class,
        dpv-owl:ContractualClauseFulfilmentStatus ;
    dct:created "2024-08-27"^^xsd:date ;
    rdfs:isDefinedBy dpv-owl: ;
    rdfs:subClassOf dpv-owl:ContractualClauseFulfilmentStatus ;
    sw:term_status "accepted"@en ;
    skos:definition "Status indicating the terms of the contractual clause have not yet been fulfiled in a manner that does not constitute a violation i.e. there is still an opportunity to complete them"@en ;
    skos:prefLabel "Contractual Clause Unfulfiled"@en .

dpv-owl:ContractualClausePartiallyFulfiled a rdfs:Class,
        owl:Class,
        dpv-owl:ContractualClauseFulfilmentStatus ;
    dct:created "2024-08-27"^^xsd:date ;
    rdfs:isDefinedBy dpv-owl: ;
    rdfs:subClassOf dpv-owl:ContractualClauseFulfilmentStatus ;
    sw:term_status "accepted"@en ;
    skos:definition "Status indicating some of the terms of the contractual clause have been fulfiled, and others have not yet been fulfiled in a manner that does not constitute a violation i.e. there is still an opportunity to complete them"@en ;
    skos:prefLabel "Contractual Clause Partially Fulfiled"@en .

dpv-owl:ContractualClauseViolated a rdfs:Class,
        owl:Class,
        dpv-owl:ContractualClauseFulfilmentStatus ;
    dct:created "2024-08-27"^^xsd:date ;
    rdfs:isDefinedBy dpv-owl: ;
    rdfs:subClassOf dpv-owl:ContractualClauseFulfilmentStatus ;
    sw:term_status "accepted"@en ;
    skos:definition "Status indicating the terms of the contractual clause have been violated"@en ;
    skos:prefLabel "Contractual Clause Breached"@en .

dpv-owl:TermsOfService a rdfs:Class,
        owl:Class,
        dpv-owl:ContractualClause ;
    dct:contributor _:N05cd1f43dbaf4b4ba297dab5ee221394 ;
    dct:created "2024-08-27"^^xsd:date ;
    rdfs:isDefinedBy dpv-owl: ;
    rdfs:subClassOf dpv-owl:ContractualClause ;
    sw:term_status "accepted"@en ;
    skos:definition "Contractual clauses outlining the terms and conditions regarding the provision of a service, typically between a service provider and a service consumer, also know as 'Terms of Use' and 'Terms and Conditions' and commonly abbreviated as TOS, ToS, ToU, or T&C"@en ;
    skos:prefLabel "Terms of Service"@en .

dpv-owl:serialisation-html a profile:ResourceDescriptor ;
    dct:conformsTo <https://www.w3.org/TR/html/> ;
    dct:format <https://www.iana.org/assignments/media-types/text/html> ;
    dct:title "Data Privacy Vocabulary (DPV) - HTML serialiation" ;
    profile:hasArtifact <https://w3id.org/dpv/dpv-owl.html> ;
    profile:hasRole role:specification .

dpv-owl:serialisation-jsonld a profile:ResourceDescriptor ;
    dct:conformsTo <https://www.w3.org/TR/json-ld11/> ;
    dct:format <https://www.iana.org/assignments/media-types/application/ld+json> ;
    dct:title "Data Privacy Vocabulary (DPV) - JSON-LD serialiation" ;
    profile:hasArtifact <https://w3id.org/dpv/dpv/dpv-owl.jsonld> ;
    profile:hasRole role:vocabulary .

dpv-owl:serialisation-n3 a profile:ResourceDescriptor ;
    dct:conformsTo <https://www.w3.org/TeamSubmission/n3/> ;
    dct:format <https://www.iana.org/assignments/media-types/text/n3> ;
    dct:title "Data Privacy Vocabulary (DPV) - N3 serialiation" ;
    profile:hasArtifact <https://w3id.org/dpv/dpv/dpv-owl.n3> ;
    profile:hasRole role:vocabulary .

dpv-owl:serialisation-rdf a profile:ResourceDescriptor ;
    dct:conformsTo rdf: ;
    dct:format <https://www.iana.org/assignments/media-types/application/rdf+xml> ;
    dct:title "Data Privacy Vocabulary (DPV) - RDF/XML serialiation" ;
    profile:hasArtifact <https://w3id.org/dpv/dpv/dpv-owl.rdf> ;
    profile:hasRole role:vocabulary .

dpv-owl:serialisation-ttl a profile:ResourceDescriptor ;
    dct:conformsTo <https://www.w3.org/TR/turtle/> ;
    dct:format <https://www.iana.org/assignments/media-types/text/turtle> ;
    dct:title "Data Privacy Vocabulary (DPV) - Turtle serialiation" ;
    profile:hasArtifact <https://w3id.org/dpv/dpv/dpv-owl.ttl> ;
    profile:hasRole role:vocabulary .

<https://w3id.org/dpv/examples> a profile:ResourceDescriptor ;
    dct:conformsTo <https://www.w3.org/TR/html/> ;
    dct:format <https://www.iana.org/assignments/media-types/text/html> ;
    dct:title "Examples for Data Privacy Vocabulary" ;
    profile:hasArtifact <https://w3id.org/dpv/examples> ;
    profile:hasRole role:guidance .

<https://w3id.org/dpv/guides> a profile:ResourceDescriptor ;
    dct:conformsTo <https://www.w3.org/TR/html/> ;
    dct:format <https://www.iana.org/assignments/media-types/text/html> ;
    dct:title "Guides for Data Privacy Vocabulary" ;
    profile:hasArtifact <https://w3id.org/dpv/guides> ;
    profile:hasRole role:guidance .

<https://w3id.org/dpv/primer> a profile:ResourceDescriptor ;
    dct:conformsTo <https://www.w3.org/TR/html/> ;
    dct:format <https://www.iana.org/assignments/media-types/text/html> ;
    dct:title "Primer for Data Privacy Vocabulary" ;
    profile:hasArtifact <https://w3id.org/dpv/primer> ;
    profile:hasRole role:guidance .

dpv-owl: a owl:Ontology,
        profile:Profile ;
    dct:bibliographicCitation "Harshvardhan J. Pandit, Beatriz Esteves, Georg P. Krog, Paul Ryan, Delaram Golpayegani, Julian Flake (2025) Data Privacy Vocabulary (DPV) – Version 2.0. In: Demartini, G., et al. The Semantic Web – ISWC 2024. ISWC 2024. Lecture Notes in Computer Science, vol 15233. Springer, Cham. https://doi.org/10.1007/978-3-031-77847-6_10" ;
    dct:conformsTo <http://www.w3.org/2002/07/owl>,
        "http://www.w3.org/2000/01/rdf-schema",
        "http://www.w3.org/2004/02/skos/core" ;
    dct:contributor _:N05cd1f43dbaf4b4ba297dab5ee221394 ;
    dct:created "2022-08-18"@en ;
    dct:creator _:N05cd1f43dbaf4b4ba297dab5ee221394,
        [ a dct:Agent,
                foaf:Person ;
            scoro:hasORCID "0000-0002-5068-3714" ;
            org:memberOf [ a foaf:Organization ;
                    foaf:name "ADAPT Centre, Dublin City University" ] ;
            foaf:homepage "https://harshp.com/" ;
            foaf:name "Harshvardhan J. Pandit" ],
        [ a dct:Agent,
                foaf:Person ;
            scoro:hasORCID "0009-0006-4623-1463" ;
            org:memberOf [ a foaf:Organization ;
                    foaf:name "University of Koblenz" ] ;
            foaf:name "Julian Flake" ],
        [ a dct:Agent,
                foaf:Person ;
            scoro:hasORCID "0000-0003-0259-7560" ;
            org:memberOf [ a foaf:Organization ;
                    foaf:name "IDLab, IMEC, Ghent University" ] ;
            foaf:name "Beatriz Esteves" ],
        [ a dct:Agent,
                foaf:Person ;
            scoro:hasORCID "0000-0003-0770-2737" ;
            org:memberOf [ a foaf:Organization ;
                    foaf:name "Uniphar PLC" ] ;
            foaf:name "Paul Ryan" ],
        [ a dct:Agent,
                foaf:Person ;
            scoro:hasORCID "0000-0002-1208-186X" ;
            org:memberOf [ a foaf:Organization ;
                    foaf:name "ADAPT Centre, Trinity College Dublin" ] ;
            foaf:name "Delaram Golpayegani" ] ;
    dct:description "The Data Privacy Vocabulary (DPV) provides terms (classes and properties) to represent information about processing of personal data, for example - purposes, processing operations, personal data, technical and organisational measures."@en ;
    dct:hasVersion dpv-owl: ;
    dct:identifier "https://w3id.org/dpv" ;
    dct:issued "2022-08-18"@en ;
    dct:license <https://www.w3.org/copyright/document-license-2023/> ;
    dct:modified "2025-03-16"@en ;
    dct:publisher <https://www.w3.org/> ;
    dct:source <https://www.w3.org/groups/cg/dpvcg/> ;
    dct:title "Data Privacy Vocabulary (DPV)"@en ;
    bibo:doi "10.5281/zenodo.12505841" ;
    bibo:status "http://purl.org/ontology/bibo/status/published" ;
    vann:preferredNamespacePrefix "dpv" ;
    vann:preferredNamespaceUri "https://w3id.org/dpv#" ;
    rdfs:Label "DPV"@en ;
    owl:versionIRI <https://w3id.org/dpv/2.1/owl#> ;
    owl:versionInfo "2.1" ;
    profile:hasResource <https://w3id.org/dpv/examples>,
        <https://w3id.org/dpv/guides>,
        dpv-owl:serialisation-html,
        dpv-owl:serialisation-jsonld,
        dpv-owl:serialisation-n3,
        dpv-owl:serialisation-rdf,
        dpv-owl:serialisation-ttl,
        <https://w3id.org/dpv/primer> ;
    profile:isProfileOf <http://www.w3.org/2002/07/owl>,
        dpv-owl: ;
    foaf:logo <https://w3id.org/dpv/media/logo.png> ;
    schema:version "2.1" .

_:N2bfb2dfcc0b24c5182bd06c242c085fa a foaf:Organization ;
    foaf:name "Signatu AS" .

_:N05cd1f43dbaf4b4ba297dab5ee221394 a dct:Agent,
        foaf:Person ;
    org:memberOf _:N2bfb2dfcc0b24c5182bd06c242c085fa ;
    foaf:homepage "https://www.linkedin.com/in/georg-philip-krog-a2a278104/" ;
    foaf:name "Georg P. Krog" .

