@prefix bibo: <http://purl.org/ontology/bibo/> .
@prefix dct: <http://purl.org/dc/terms/> .
@prefix dex-owl: <https://w3id.org/dpv/examples/owl#> .
@prefix dpv-owl: <https://w3id.org/dpv/owl#> .
@prefix foaf: <http://xmlns.com/foaf/0.1/> .
@prefix org: <http://www.w3.org/ns/org#> .
@prefix owl: <http://www.w3.org/2002/07/owl#> .
@prefix profile: <http://www.w3.org/ns/dx/prof/> .
@prefix rdf: <http://www.w3.org/1999/02/22-rdf-syntax-ns#> .
@prefix rdfs: <http://www.w3.org/2000/01/rdf-schema#> .
@prefix role: <http://www.w3.org/ns/dx/prof/role/> .
@prefix schema: <https://schema.org/> .
@prefix scoro: <http://purl.org/spar/scoro/> .
@prefix skos: <http://www.w3.org/2004/02/skos/core#> .
@prefix sw: <http://www.w3.org/2003/06/sw-vocab-status/ns#> .
@prefix vann: <http://purl.org/vocab/vann/> .
@prefix xsd: <http://www.w3.org/2001/XMLSchema#> .

dpv-owl:B2B2CContract a rdfs:Class,
        owl:Class,
        dpv-owl:LegalBasis ;
    dct:contributor _:N05cd1f43dbaf4b4ba297dab5ee221394,
        _:N458008bc6195484e9cc557f70eabda31 ;
    dct:created "2024-08-27"^^xsd:date ;
    rdfs:isDefinedBy dpv-owl: ;
    rdfs:subClassOf dpv-owl:B2BContract,
        dpv-owl:B2CContract ;
    sw:term_status "accepted"@en ;
    skos:definition "A contract between two businesses who partner together to provide services to a consumer"@en ;
    skos:prefLabel "Business-to-Business-to-Consumer Contract"@en .

dpv-owl:B2BContract a rdfs:Class,
        owl:Class,
        dpv-owl:LegalBasis ;
    dct:created "2024-08-27"^^xsd:date ;
    rdfs:isDefinedBy dpv-owl: ;
    rdfs:subClassOf dpv-owl:ContractByEntityType ;
    sw:term_status "accepted"@en ;
    skos:definition "A contract between two businesses"@en ;
    skos:prefLabel "Business-to-Business Contract"@en .

dpv-owl:B2CContract a rdfs:Class,
        owl:Class,
        dpv-owl:LegalBasis ;
    dct:created "2024-08-27"^^xsd:date ;
    rdfs:isDefinedBy dpv-owl: ;
    rdfs:subClassOf dpv-owl:ContractByEntityType ;
    sw:term_status "accepted"@en ;
    skos:definition "A contract between a business and a consumer where the business provides goods or services to the consumer"@en ;
    skos:prefLabel "Business-to-Consumer Contract"@en .

dpv-owl:C2BContract a rdfs:Class,
        owl:Class,
        dpv-owl:LegalBasis ;
    dct:created "2024-08-27"^^xsd:date ;
    rdfs:isDefinedBy dpv-owl: ;
    rdfs:subClassOf dpv-owl:ContractByEntityType ;
    sw:term_status "accepted"@en ;
    skos:definition "A contract between a consumer and a business where the business purchases goods or services from the consumer"@en ;
    skos:prefLabel "Consumer-to-Business Contract"@en .

dpv-owl:C2CContract a rdfs:Class,
        owl:Class,
        dpv-owl:LegalBasis ;
    dct:created "2024-08-27"^^xsd:date ;
    rdfs:isDefinedBy dpv-owl: ;
    rdfs:subClassOf dpv-owl:ContractByEntityType ;
    sw:term_status "accepted"@en ;
    skos:definition "A contract between two consumers"@en ;
    skos:prefLabel "Consumer-to-Consumer Contract"@en .

dpv-owl:ConsumerStandardFormContract a rdfs:Class,
        owl:Class,
        dpv-owl:LegalBasis ;
    dct:created "2024-08-27"^^xsd:date ;
    rdfs:isDefinedBy dpv-owl: ;
    rdfs:subClassOf dpv-owl:StandardFormContract ;
    sw:term_status "accepted"@en ;
    skos:definition "A contract where the terms and conditions are determined by parties in the role of a 'consumer' - whether an entity or an individual, and the other parties have negligible or no ability to negotiate the terms and conditions"@en ;
    skos:prefLabel "Consumer Standard Form Contract"@en .

dpv-owl:ContractByDomain a rdfs:Class,
        owl:Class,
        dpv-owl:LegalBasis ;
    dct:created "2024-12-17"^^xsd:date ;
    rdfs:isDefinedBy dpv-owl: ;
    rdfs:subClassOf dpv-owl:Contract ;
    sw:term_status "accepted"@en ;
    skos:definition "A generic concept representing contracts categorised by specific domains which dictate the drafting and interpretation of contracts"@en ;
    skos:prefLabel "Contract by Domain"@en .

dpv-owl:ContractByEntityType a rdfs:Class,
        owl:Class,
        dpv-owl:LegalBasis ;
    dct:created "2024-12-17"^^xsd:date ;
    rdfs:isDefinedBy dpv-owl: ;
    rdfs:subClassOf dpv-owl:Contract ;
    sw:term_status "accepted"@en ;
    skos:definition "A generic concept representing contracts categorised by the type of entities involved - such as Businesses (B), Consumers (C), and Governments (G)"@en ;
    skos:prefLabel "Contract by Entity Type"@en .

dpv-owl:ContractByNegotiationType a rdfs:Class,
        owl:Class,
        dpv-owl:LegalBasis ;
    dct:created "2024-12-17"^^xsd:date ;
    rdfs:isDefinedBy dpv-owl: ;
    rdfs:subClassOf dpv-owl:Contract ;
    sw:term_status "accepted"@en ;
    skos:definition "A generic concept representing contracts categorised based on their use or absence of negotiation in the contract forming process"@en ;
    skos:prefLabel "Contract by Negotiation Type"@en .

dpv-owl:ControllerDataSubjectAgreement a rdfs:Class,
        owl:Class,
        dpv-owl:LegalBasis,
        dpv-owl:LegalMeasure ;
    dct:created "2024-08-27"^^xsd:date ;
    dct:modified "2024-08-27"^^xsd:date ;
    rdfs:isDefinedBy dpv-owl: ;
    rdfs:subClassOf dpv-owl:DataSubjectContract ;
    sw:term_status "modified"@en ;
    skos:definition "An agreement outlining conditions, criteria, obligations, responsibilities, and specifics for carrying out processing of data between a Data Controller and a Data Subject"@en ;
    skos:prefLabel "Controller-Data Subject Agreement"@en .

dpv-owl:ControllerProcessorAgreement a rdfs:Class,
        owl:Class,
        dpv-owl:LegalBasis,
        dpv-owl:LegalMeasure ;
    dct:contributor _:N05cd1f43dbaf4b4ba297dab5ee221394,
        _:N0a43dd9ea5e94fe695d8b7df8802cfdd,
        _:N0c29df1c09e34406bfb949a8e7afb527,
        _:N458008bc6195484e9cc557f70eabda31,
        _:Nd0960ac69a57403fb5db2455be10d160 ;
    dct:created "2022-01-26"^^xsd:date ;
    dct:modified "2024-08-27"^^xsd:date ;
    vann:example dex-owl:E0024 ;
    rdfs:isDefinedBy dpv-owl: ;
    rdfs:subClassOf dpv-owl:DataProcessorContract ;
    sw:term_status "modified"@en ;
    skos:definition "An agreement outlining conditions, criteria, obligations, responsibilities, and specifics for carrying out processing of data between a Data Controller and a Data Processor"@en ;
    skos:prefLabel "Controller-Processor Agreement"@en .

dpv-owl:DataControllerContract a rdfs:Class,
        owl:Class,
        dpv-owl:LegalBasis ;
    dct:created "2023-12-10"^^xsd:date ;
    dct:modified "2024-08-27"^^xsd:date ;
    rdfs:isDefinedBy dpv-owl: ;
    rdfs:subClassOf dpv-owl:DataProcessingAgreement ;
    sw:term_status "sunset"@en ;
    skos:definition "Creation, completion, fulfilment, or performance of a contract, with Data Controllers as parties being Joint Data Controllers, and involving specified processing of data or technologies. NOTE: This concept is being deprecated - use dpv:JointDataControllersAgreement which has a more explicit definition of the entities involved and the intent of the contract"@en ;
    skos:prefLabel "Data Controller Contract"@en .

dpv-owl:DataProcessingAgreement a rdfs:Class,
        owl:Class,
        dpv-owl:LegalBasis,
        dpv-owl:LegalMeasure ;
    dct:contributor _:N05cd1f43dbaf4b4ba297dab5ee221394,
        _:N0a43dd9ea5e94fe695d8b7df8802cfdd,
        _:N0c29df1c09e34406bfb949a8e7afb527,
        _:N458008bc6195484e9cc557f70eabda31,
        _:Nd0960ac69a57403fb5db2455be10d160 ;
    dct:created "2022-01-26"^^xsd:date ;
    dct:modified "2024-12-17"^^xsd:date ;
    rdfs:isDefinedBy dpv-owl: ;
    rdfs:subClassOf dpv-owl:Contract ;
    sw:term_status "modified"@en ;
    skos:definition "An agreement outlining conditions, criteria, obligations, responsibilities, and specifics for carrying out processing of data"@en ;
    skos:prefLabel "Data Processing Agreement"@en ;
    skos:scopeNote "For specific role-based data processing agreements, see concepts for Processors and JointDataController agreements."@en .

dpv-owl:DataProcessorContract a rdfs:Class,
        owl:Class,
        dpv-owl:LegalBasis ;
    dct:created "2023-12-10"^^xsd:date ;
    dct:modified "2024-08-27"^^xsd:date ;
    rdfs:isDefinedBy dpv-owl: ;
    rdfs:subClassOf dpv-owl:DataProcessingAgreement ;
    sw:term_status "sunset"@en ;
    skos:definition "Creation, completion, fulfilment, or performance of a contract, with the Data Controller and Data Processor as parties, and involving specified processing of data or technologies. NOTE: This concept is being deprecated - use dpv:ControllerProcessorAgreement which has a more explicit definition of the entities involved and the intent of the contract"@en ;
    skos:prefLabel "Data Processor Contract"@en .

dpv-owl:DataSubjectContract a rdfs:Class,
        owl:Class,
        dpv-owl:LegalBasis ;
    dct:created "2023-12-10"^^xsd:date ;
    dct:modified "2024-08-27"^^xsd:date ;
    rdfs:isDefinedBy dpv-owl: ;
    rdfs:subClassOf dpv-owl:DataProcessingAgreement ;
    sw:term_status "sunset"@en ;
    skos:definition "Creation, completion, fulfilment, or performance of a contract, with the Data Controller and Data Subject as parties, and involving specified processing of data or technologies. NOTE: This concept is being deprecated - use dpv:ControllerDataSubjectAgreement which has a more explicit definition of the entities involved and the intent of the contract"@en ;
    skos:prefLabel "Data Subject Contract"@en .

dpv-owl:DistributionAgreement a rdfs:Class,
        owl:Class,
        dpv-owl:LegalBasis ;
    dct:created "2024-08-27"^^xsd:date ;
    rdfs:isDefinedBy dpv-owl: ;
    rdfs:subClassOf dpv-owl:ContractByDomain ;
    sw:term_status "accepted"@en ;
    skos:definition "A contract regarding supply of data or technologies between a distributor and a supplier"@en ;
    skos:prefLabel "Distribution Agreement"@en .

dpv-owl:EULA a rdfs:Class,
        owl:Class,
        dpv-owl:LegalBasis ;
    dct:created "2024-08-27"^^xsd:date ;
    rdfs:isDefinedBy dpv-owl: ;
    rdfs:subClassOf dpv-owl:LicenseAgreement ;
    sw:term_status "accepted"@en ;
    skos:definition "End User License Agreement is a contract entered into between a software (or service) developer or provider with the (end-)user"@en ;
    skos:prefLabel "End User License Agreement (EULA)"@en .

dpv-owl:EmploymentContract a rdfs:Class,
        owl:Class,
        dpv-owl:LegalBasis ;
    dct:created "2024-08-27"^^xsd:date ;
    rdfs:isDefinedBy dpv-owl: ;
    rdfs:subClassOf dpv-owl:ContractByDomain ;
    sw:term_status "accepted"@en ;
    skos:definition "A contract regarding employment between an employer and an employee"@en ;
    skos:prefLabel "Employment Contract"@en .

dpv-owl:G2BContract a rdfs:Class,
        owl:Class,
        dpv-owl:LegalBasis ;
    dct:created "2024-08-27"^^xsd:date ;
    rdfs:isDefinedBy dpv-owl: ;
    rdfs:subClassOf dpv-owl:ContractByEntityType ;
    sw:term_status "accepted"@en ;
    skos:definition "A contract between a government and a business"@en ;
    skos:prefLabel "Government-to-Business Contract"@en .

dpv-owl:G2CContract a rdfs:Class,
        owl:Class,
        dpv-owl:LegalBasis ;
    dct:created "2024-08-27"^^xsd:date ;
    rdfs:isDefinedBy dpv-owl: ;
    rdfs:subClassOf dpv-owl:ContractByEntityType ;
    sw:term_status "accepted"@en ;
    skos:definition "A contract between a government and consumers"@en ;
    skos:prefLabel "Government-to-Consumer Contract"@en .

dpv-owl:G2GContract a rdfs:Class,
        owl:Class,
        dpv-owl:LegalBasis ;
    dct:created "2024-08-27"^^xsd:date ;
    rdfs:isDefinedBy dpv-owl: ;
    rdfs:subClassOf dpv-owl:ContractByEntityType ;
    sw:term_status "accepted"@en ;
    skos:definition "A contract between two governments or government departments or units"@en ;
    skos:prefLabel "Government-to-Government Contract"@en .

dpv-owl:JointDataControllersAgreement a rdfs:Class,
        owl:Class,
        dpv-owl:LegalBasis,
        dpv-owl:LegalMeasure ;
    dct:contributor _:N05cd1f43dbaf4b4ba297dab5ee221394,
        _:N0a43dd9ea5e94fe695d8b7df8802cfdd,
        _:N0c29df1c09e34406bfb949a8e7afb527,
        _:N458008bc6195484e9cc557f70eabda31,
        _:Nd0960ac69a57403fb5db2455be10d160 ;
    dct:created "2022-01-26"^^xsd:date ;
    dct:modified "2024-08-27"^^xsd:date ;
    rdfs:isDefinedBy dpv-owl: ;
    rdfs:subClassOf dpv-owl:DataControllerContract ;
    sw:term_status "modified"@en ;
    skos:definition "An agreement outlining conditions, criteria, obligations, responsibilities, and specifics for carrying out processing of data between Controllers within a Joint Controllers relationship"@en ;
    skos:prefLabel "Joint Data Controllers Agreement"@en .

dpv-owl:LicenseAgreement a rdfs:Class,
        owl:Class,
        dpv-owl:LegalBasis ;
    dct:created "2024-08-27"^^xsd:date ;
    rdfs:isDefinedBy dpv-owl: ;
    rdfs:subClassOf dpv-owl:ContractByDomain ;
    sw:term_status "accepted"@en ;
    skos:definition "A Legal Document providing permission to utilise data or resource and outlining the conditions under which such use is considered valid"@en ;
    skos:prefLabel "License Agreement"@en .

dpv-owl:NegotiatedContract a rdfs:Class,
        owl:Class,
        dpv-owl:LegalBasis ;
    dct:created "2024-08-27"^^xsd:date ;
    rdfs:isDefinedBy dpv-owl: ;
    rdfs:subClassOf dpv-owl:ContractByNegotiationType ;
    sw:term_status "accepted"@en ;
    skos:definition "A contract where the terms and conditions are determined with all parties having the ability to negotiate the terms and conditions"@en ;
    skos:prefLabel "Negotiated Contract"@en ;
    skos:scopeNote "Negotiation here refers to the opportunity for a party on their own initiative to modify or dictate terms and conditions within a contract. If the party is provided a set of options to choose from or in other ways is dictated which terms and conditions can be present in the contract, neither of these should be considered a negotiation"@en .

dpv-owl:ProviderStandardFormContract a rdfs:Class,
        owl:Class,
        dpv-owl:LegalBasis ;
    dct:created "2024-08-27"^^xsd:date ;
    rdfs:isDefinedBy dpv-owl: ;
    rdfs:subClassOf dpv-owl:StandardFormContract ;
    sw:term_status "accepted"@en ;
    skos:definition "A contract where the terms and conditions are determined by parties in the role of a 'provider', and the other parties have negligible or no ability to negotiate the terms and conditions"@en ;
    skos:prefLabel "Provider Standard Form Contract"@en .

dpv-owl:ServiceLevelAgreement a rdfs:Class,
        owl:Class,
        dpv-owl:LegalBasis ;
    dct:created "2024-08-27"^^xsd:date ;
    rdfs:isDefinedBy dpv-owl: ;
    rdfs:subClassOf dpv-owl:ContractByDomain ;
    sw:term_status "accepted"@en ;
    skos:definition "A contract regarding the provision of a service which outlines the acceptable metrics and performance of the service for the consumer"@en ;
    skos:prefLabel "Service Legvel Agreement (SLA)"@en .

dpv-owl:StandardFormContract a rdfs:Class,
        owl:Class,
        dpv-owl:LegalBasis ;
    dct:created "2024-08-27"^^xsd:date ;
    rdfs:isDefinedBy dpv-owl: ;
    rdfs:subClassOf dpv-owl:ContractByNegotiationType ;
    sw:term_status "accepted"@en ;
    skos:definition "A contract where the terms and conditions are determined by one or more of the parties, and the other parties have negligible or no ability to negotiate the terms and conditions"@en ;
    skos:prefLabel "Standard Form Contract"@en ;
    skos:scopeNote "Such a contract results in the unempowered parties being in a \"take it or leave it\" position as they can only accept or reject the contract. Standard form contracts are also known as \"Adhesion contract\" or \"Boilerplate contract\""@en .

dpv-owl:SubProcessorAgreement a rdfs:Class,
        owl:Class,
        dpv-owl:LegalBasis,
        dpv-owl:LegalMeasure ;
    dct:contributor _:N05cd1f43dbaf4b4ba297dab5ee221394,
        _:N0a43dd9ea5e94fe695d8b7df8802cfdd,
        _:N0c29df1c09e34406bfb949a8e7afb527,
        _:N458008bc6195484e9cc557f70eabda31,
        _:Nd0960ac69a57403fb5db2455be10d160 ;
    dct:created "2022-01-26"^^xsd:date ;
    dct:modified "2024-08-27"^^xsd:date ;
    rdfs:isDefinedBy dpv-owl: ;
    rdfs:subClassOf dpv-owl:DataProcessingAgreement ;
    sw:term_status "modified"@en ;
    skos:definition "An agreement outlining conditions, criteria, obligations, responsibilities, and specifics for carrying out processing of data between a Data Processor and a Data (Sub-)Processor"@en ;
    skos:prefLabel "Sub-Processor Agreement"@en .

dpv-owl:ThirdPartyAgreement a rdfs:Class,
        owl:Class,
        dpv-owl:LegalBasis,
        dpv-owl:LegalMeasure ;
    dct:contributor _:N0a43dd9ea5e94fe695d8b7df8802cfdd ;
    dct:created "2022-02-09"^^xsd:date ;
    dct:modified "2024-08-27"^^xsd:date ;
    rdfs:isDefinedBy dpv-owl: ;
    rdfs:subClassOf dpv-owl:ThirdPartyContract ;
    sw:term_status "modified"@en ;
    skos:definition "An agreement outlining conditions, criteria, obligations, responsibilities, and specifics for carrying out processing of data between a Data Controller or Processor and a Third Party"@en ;
    skos:prefLabel "Third-Party Agreement"@en .

dpv-owl:ThirdPartyContract a rdfs:Class,
        owl:Class,
        dpv-owl:LegalBasis ;
    dct:created "2023-12-10"^^xsd:date ;
    dct:modified "2024-08-27"^^xsd:date ;
    rdfs:isDefinedBy dpv-owl: ;
    rdfs:subClassOf dpv-owl:DataProcessingAgreement ;
    sw:term_status "sunset"@en ;
    skos:definition "Creation, completion, fulfilment, or performance of a contract, with the Data Controller and Third Party as parties, and involving specified processing of data or technologies. NOTE: This concept is being deprecated - use dpv:ThirdPartyAgreement which has a more explicit definition of the entities involved and the intent of the contract"@en ;
    skos:prefLabel "Third Party Contract"@en .

dpv-owl:serialisation-html a profile:ResourceDescriptor ;
    dct:conformsTo <https://www.w3.org/TR/html/> ;
    dct:format <https://www.iana.org/assignments/media-types/text/html> ;
    dct:title "Data Privacy Vocabulary (DPV) - HTML serialiation" ;
    profile:hasArtifact <https://w3id.org/dpv/dpv-owl.html> ;
    profile:hasRole role:specification .

dpv-owl:serialisation-jsonld a profile:ResourceDescriptor ;
    dct:conformsTo <https://www.w3.org/TR/json-ld11/> ;
    dct:format <https://www.iana.org/assignments/media-types/application/ld+json> ;
    dct:title "Data Privacy Vocabulary (DPV) - JSON-LD serialiation" ;
    profile:hasArtifact <https://w3id.org/dpv/dpv/dpv-owl.jsonld> ;
    profile:hasRole role:vocabulary .

dpv-owl:serialisation-n3 a profile:ResourceDescriptor ;
    dct:conformsTo <https://www.w3.org/TeamSubmission/n3/> ;
    dct:format <https://www.iana.org/assignments/media-types/text/n3> ;
    dct:title "Data Privacy Vocabulary (DPV) - N3 serialiation" ;
    profile:hasArtifact <https://w3id.org/dpv/dpv/dpv-owl.n3> ;
    profile:hasRole role:vocabulary .

dpv-owl:serialisation-rdf a profile:ResourceDescriptor ;
    dct:conformsTo rdf: ;
    dct:format <https://www.iana.org/assignments/media-types/application/rdf+xml> ;
    dct:title "Data Privacy Vocabulary (DPV) - RDF/XML serialiation" ;
    profile:hasArtifact <https://w3id.org/dpv/dpv/dpv-owl.rdf> ;
    profile:hasRole role:vocabulary .

dpv-owl:serialisation-ttl a profile:ResourceDescriptor ;
    dct:conformsTo <https://www.w3.org/TR/turtle/> ;
    dct:format <https://www.iana.org/assignments/media-types/text/turtle> ;
    dct:title "Data Privacy Vocabulary (DPV) - Turtle serialiation" ;
    profile:hasArtifact <https://w3id.org/dpv/dpv/dpv-owl.ttl> ;
    profile:hasRole role:vocabulary .

<https://w3id.org/dpv/examples> a profile:ResourceDescriptor ;
    dct:conformsTo <https://www.w3.org/TR/html/> ;
    dct:format <https://www.iana.org/assignments/media-types/text/html> ;
    dct:title "Examples for Data Privacy Vocabulary" ;
    profile:hasArtifact <https://w3id.org/dpv/examples> ;
    profile:hasRole role:guidance .

<https://w3id.org/dpv/guides> a profile:ResourceDescriptor ;
    dct:conformsTo <https://www.w3.org/TR/html/> ;
    dct:format <https://www.iana.org/assignments/media-types/text/html> ;
    dct:title "Guides for Data Privacy Vocabulary" ;
    profile:hasArtifact <https://w3id.org/dpv/guides> ;
    profile:hasRole role:guidance .

<https://w3id.org/dpv/primer> a profile:ResourceDescriptor ;
    dct:conformsTo <https://www.w3.org/TR/html/> ;
    dct:format <https://www.iana.org/assignments/media-types/text/html> ;
    dct:title "Primer for Data Privacy Vocabulary" ;
    profile:hasArtifact <https://w3id.org/dpv/primer> ;
    profile:hasRole role:guidance .

dpv-owl: a owl:Ontology,
        profile:Profile ;
    dct:bibliographicCitation "Harshvardhan J. Pandit, Beatriz Esteves, Georg P. Krog, Paul Ryan, Delaram Golpayegani, Julian Flake (2025) Data Privacy Vocabulary (DPV) – Version 2.0. In: Demartini, G., et al. The Semantic Web – ISWC 2024. ISWC 2024. Lecture Notes in Computer Science, vol 15233. Springer, Cham. https://doi.org/10.1007/978-3-031-77847-6_10" ;
    dct:conformsTo <http://www.w3.org/2002/07/owl>,
        "http://www.w3.org/2000/01/rdf-schema",
        "http://www.w3.org/2004/02/skos/core" ;
    dct:contributor _:N05cd1f43dbaf4b4ba297dab5ee221394,
        _:N0a43dd9ea5e94fe695d8b7df8802cfdd,
        _:N0c29df1c09e34406bfb949a8e7afb527,
        _:N458008bc6195484e9cc557f70eabda31,
        _:Nd0960ac69a57403fb5db2455be10d160 ;
    dct:created "2022-08-18"@en ;
    dct:creator _:N05cd1f43dbaf4b4ba297dab5ee221394,
        _:N0a43dd9ea5e94fe695d8b7df8802cfdd,
        _:N0c29df1c09e34406bfb949a8e7afb527,
        _:N458008bc6195484e9cc557f70eabda31,
        _:Nd0960ac69a57403fb5db2455be10d160,
        [ a dct:Agent,
                foaf:Person ;
            scoro:hasORCID "0000-0002-1208-186X" ;
            org:memberOf [ a foaf:Organization ;
                    foaf:name "ADAPT Centre, Trinity College Dublin" ] ;
            foaf:name "Delaram Golpayegani" ] ;
    dct:description "The Data Privacy Vocabulary (DPV) provides terms (classes and properties) to represent information about processing of personal data, for example - purposes, processing operations, personal data, technical and organisational measures."@en ;
    dct:hasVersion dpv-owl: ;
    dct:identifier "https://w3id.org/dpv" ;
    dct:issued "2022-08-18"@en ;
    dct:license <https://www.w3.org/copyright/document-license-2023/> ;
    dct:modified "2025-03-16"@en ;
    dct:publisher <https://www.w3.org/> ;
    dct:source <https://www.w3.org/groups/cg/dpvcg/> ;
    dct:title "Data Privacy Vocabulary (DPV)"@en ;
    bibo:doi "10.5281/zenodo.12505841" ;
    bibo:status "http://purl.org/ontology/bibo/status/published" ;
    vann:preferredNamespacePrefix "dpv" ;
    vann:preferredNamespaceUri "https://w3id.org/dpv#" ;
    rdfs:Label "DPV"@en ;
    owl:versionIRI <https://w3id.org/dpv/2.1/owl#> ;
    owl:versionInfo "2.1" ;
    profile:hasResource <https://w3id.org/dpv/examples>,
        <https://w3id.org/dpv/guides>,
        dpv-owl:serialisation-html,
        dpv-owl:serialisation-jsonld,
        dpv-owl:serialisation-n3,
        dpv-owl:serialisation-rdf,
        dpv-owl:serialisation-ttl,
        <https://w3id.org/dpv/primer> ;
    profile:isProfileOf <http://www.w3.org/2002/07/owl>,
        dpv-owl: ;
    foaf:logo <https://w3id.org/dpv/media/logo.png> ;
    schema:version "2.1" .

_:N2bfb2dfcc0b24c5182bd06c242c085fa a foaf:Organization ;
    foaf:name "Signatu AS" .

_:N313d89a6c37147bfac1bbb4aa7f6510b a foaf:Organization ;
    foaf:name "ADAPT Centre, Dublin City University" .

_:N3f64d3533a104953b63bb217ff4665c5 a foaf:Organization ;
    foaf:name "IDLab, IMEC, Ghent University" .

_:N77a9e87e7f0e42959387d0b6a299325f a foaf:Organization ;
    foaf:name "Uniphar PLC" .

_:Nd69451d3e8ae4c24b46f61e344aae1e2 a foaf:Organization ;
    foaf:name "University of Koblenz" .

_:N0c29df1c09e34406bfb949a8e7afb527 a dct:Agent,
        foaf:Person ;
    scoro:hasORCID "0009-0006-4623-1463" ;
    org:memberOf _:Nd69451d3e8ae4c24b46f61e344aae1e2 ;
    foaf:name "Julian Flake" .

_:Nd0960ac69a57403fb5db2455be10d160 a dct:Agent,
        foaf:Person ;
    scoro:hasORCID "0000-0003-0770-2737" ;
    org:memberOf _:N77a9e87e7f0e42959387d0b6a299325f ;
    foaf:name "Paul Ryan" .

_:N05cd1f43dbaf4b4ba297dab5ee221394 a dct:Agent,
        foaf:Person ;
    org:memberOf _:N2bfb2dfcc0b24c5182bd06c242c085fa ;
    foaf:homepage "https://www.linkedin.com/in/georg-philip-krog-a2a278104/" ;
    foaf:name "Georg P. Krog" .

_:N0a43dd9ea5e94fe695d8b7df8802cfdd a dct:Agent,
        foaf:Person ;
    scoro:hasORCID "0000-0002-5068-3714" ;
    org:memberOf _:N313d89a6c37147bfac1bbb4aa7f6510b ;
    foaf:homepage "https://harshp.com/" ;
    foaf:name "Harshvardhan J. Pandit" .

_:N458008bc6195484e9cc557f70eabda31 a dct:Agent,
        foaf:Person ;
    scoro:hasORCID "0000-0003-0259-7560" ;
    org:memberOf _:N3f64d3533a104953b63bb217ff4665c5 ;
    foaf:name "Beatriz Esteves" .

