@prefix bibo: <http://purl.org/ontology/bibo/> .
@prefix dcam: <http://purl.org/dc/dcam/> .
@prefix dct: <http://purl.org/dc/terms/> .
@prefix dex: <https://w3id.org/dpv/examples#> .
@prefix dpv: <https://w3id.org/dpv#> .
@prefix foaf: <http://xmlns.com/foaf/0.1/> .
@prefix org: <http://www.w3.org/ns/org#> .
@prefix owl: <http://www.w3.org/2002/07/owl#> .
@prefix profile: <http://www.w3.org/ns/dx/prof/> .
@prefix rdf: <http://www.w3.org/1999/02/22-rdf-syntax-ns#> .
@prefix rdfs: <http://www.w3.org/2000/01/rdf-schema#> .
@prefix role: <http://www.w3.org/ns/dx/prof/role/> .
@prefix schema: <https://schema.org/> .
@prefix scoro: <http://purl.org/spar/scoro/> .
@prefix skos: <http://www.w3.org/2004/02/skos/core#> .
@prefix sw: <http://www.w3.org/2003/06/sw-vocab-status/ns#> .
@prefix vann: <http://purl.org/vocab/vann/> .
@prefix xsd: <http://www.w3.org/2001/XMLSchema#> .

dpv:ConsentNotice a rdfs:Class,
        skos:Concept,
        dpv:OrganisationalMeasure ;
    dct:contributor _:N05cd1f43dbaf4b4ba297dab5ee221394,
        _:N0a43dd9ea5e94fe695d8b7df8802cfdd,
        _:N0c29df1c09e34406bfb949a8e7afb527,
        _:Nd0960ac69a57403fb5db2455be10d160 ;
    dct:created "2022-06-21"^^xsd:date ;
    vann:example dex:E0072 ;
    rdfs:isDefinedBy dpv: ;
    sw:term_status "accepted"@en ;
    skos:broader dpv:PrivacyNotice ;
    skos:definition "A Notice for information provision associated with Consent"@en ;
    skos:inScheme dpv:notice-classes ;
    skos:prefLabel "Consent Notice"@en .

dpv:DashboardNotice a rdfs:Class,
        skos:Concept,
        dpv:OrganisationalMeasure ;
    dct:created "2024-08-17"^^xsd:date ;
    dct:source [ a schema:WebPage ;
            schema:name "ICO - What methods can we use to provide privacy information?" ;
            schema:url "https://ico.org.uk/for-organisations/uk-gdpr-guidance-and-resources/individual-rights/the-right-to-be-informed/what-methods-can-we-use-to-provide-privacy-information/" ] ;
    rdfs:isDefinedBy dpv: ;
    sw:term_status "accepted"@en ;
    skos:broader dpv:Notice ;
    skos:definition "A notice that is provided within a dashboard also used for other purposes"@en ;
    skos:inScheme dpv:notice-classes ;
    skos:prefLabel "Dashboard Notice"@en .

dpv:DataBreachNotice a rdfs:Class,
        skos:Concept,
        dpv:OrganisationalMeasure ;
    dct:contributor _:N05cd1f43dbaf4b4ba297dab5ee221394,
        _:N0a43dd9ea5e94fe695d8b7df8802cfdd,
        _:N1aa8f48a4f3a40e6a438f71be918d3a1,
        _:N458008bc6195484e9cc557f70eabda31,
        _:Nd0960ac69a57403fb5db2455be10d160 ;
    dct:created "2024-04-14"^^xsd:date ;
    dct:source " DGA 21.5 GDPR 33"@en,
        " GDPR 34"@en,
        "DGA 12.k"@en ;
    rdfs:isDefinedBy dpv: ;
    sw:term_status "accepted"@en ;
    skos:broader dpv:SecurityIncidentNotice ;
    skos:definition "A notice providing information about data breach(es) i.e. unauthorised transfer, access, use, or modification of data"@en ;
    skos:inScheme dpv:notice-classes ;
    skos:prefLabel "Data Breach Notice"@en .

dpv:DataTransferNotice a rdfs:Class,
        skos:Concept,
        dpv:OrganisationalMeasure ;
    dct:contributor _:N05cd1f43dbaf4b4ba297dab5ee221394,
        _:N0a43dd9ea5e94fe695d8b7df8802cfdd,
        _:N1aa8f48a4f3a40e6a438f71be918d3a1,
        _:N458008bc6195484e9cc557f70eabda31,
        _:Nd0960ac69a57403fb5db2455be10d160 ;
    dct:created "2024-04-14"^^xsd:date ;
    dct:source "DGA 5.9"@en ;
    rdfs:isDefinedBy dpv: ;
    sw:term_status "accepted"@en ;
    skos:broader dpv:Notice ;
    skos:definition "Notice for the legal entity for the transfer of its data"@en ;
    skos:inScheme dpv:notice-classes ;
    skos:prefLabel "Data Transfer Notice"@en .

dpv:DeviceNotice a rdfs:Class,
        skos:Concept,
        dpv:OrganisationalMeasure ;
    dct:created "2024-08-17"^^xsd:date ;
    dct:source [ a schema:WebPage ;
            schema:name "ICO - What methods can we use to provide privacy information?" ;
            schema:url "https://ico.org.uk/for-organisations/uk-gdpr-guidance-and-resources/individual-rights/the-right-to-be-informed/what-methods-can-we-use-to-provide-privacy-information/" ] ;
    rdfs:isDefinedBy dpv: ;
    sw:term_status "accepted"@en ;
    skos:broader dpv:Notice ;
    skos:definition "A notice provided using the functionality provided by a device e.g. using the popup or alert feature"@en ;
    skos:inScheme dpv:notice-classes ;
    skos:prefLabel "Device Notice"@en .

dpv:GraphicalNotice a rdfs:Class,
        skos:Concept,
        dpv:OrganisationalMeasure ;
    dct:created "2024-08-17"^^xsd:date ;
    dct:source [ a schema:WebPage ;
            schema:name "ICO - What methods can we use to provide privacy information?" ;
            schema:url "https://ico.org.uk/for-organisations/uk-gdpr-guidance-and-resources/individual-rights/the-right-to-be-informed/what-methods-can-we-use-to-provide-privacy-information/" ] ;
    rdfs:isDefinedBy dpv: ;
    sw:term_status "accepted"@en ;
    skos:broader dpv:Notice ;
    skos:definition "A notice that uses graphical elements such as visualisations and icons"@en ;
    skos:inScheme dpv:notice-classes ;
    skos:prefLabel "Graphical Notice"@en .

dpv:JITNotice a rdfs:Class,
        skos:Concept,
        dpv:OrganisationalMeasure ;
    dct:created "2024-08-17"^^xsd:date ;
    dct:source [ a schema:WebPage ;
            schema:name "ICO - What methods can we use to provide privacy information?" ;
            schema:url "https://ico.org.uk/for-organisations/uk-gdpr-guidance-and-resources/individual-rights/the-right-to-be-informed/what-methods-can-we-use-to-provide-privacy-information/" ] ;
    rdfs:isDefinedBy dpv: ;
    sw:term_status "accepted"@en ;
    skos:broader dpv:Notice ;
    skos:definition "A notice that is provided \"just in time\" when collecting information or performing an activity"@en ;
    skos:inScheme dpv:notice-classes ;
    skos:prefLabel "Just-in-time Notice"@en .

dpv:LayeredNotice a rdfs:Class,
        skos:Concept,
        dpv:OrganisationalMeasure ;
    dct:created "2024-08-17"^^xsd:date ;
    dct:source [ a schema:WebPage ;
            schema:name "ICO - What methods can we use to provide privacy information?" ;
            schema:url "https://ico.org.uk/for-organisations/uk-gdpr-guidance-and-resources/individual-rights/the-right-to-be-informed/what-methods-can-we-use-to-provide-privacy-information/" ] ;
    rdfs:isDefinedBy dpv: ;
    sw:term_status "accepted"@en ;
    skos:broader dpv:Notice ;
    skos:definition "A notice that contains layered elements"@en ;
    skos:inScheme dpv:notice-classes ;
    skos:prefLabel "Layered Notice"@en .

dpv:Notice a rdfs:Class,
        skos:Concept,
        dpv:OrganisationalMeasure ;
    dct:contributor _:N05cd1f43dbaf4b4ba297dab5ee221394,
        _:N0a43dd9ea5e94fe695d8b7df8802cfdd,
        _:N1aa8f48a4f3a40e6a438f71be918d3a1,
        _:Nd0960ac69a57403fb5db2455be10d160 ;
    dct:created "2021-09-08"^^xsd:date ;
    vann:example dex:E0017 ;
    rdfs:isDefinedBy dpv: ;
    sw:term_status "accepted"@en ;
    skos:broader dpv:OrganisationalMeasure ;
    skos:definition "A notice is an artefact for providing information, choices, or controls"@en ;
    skos:inScheme dpv:notice-classes ;
    skos:prefLabel "Notice"@en ;
    skos:scopeNote "Notice refers to the information whereas Notification refers to the provision of that notice. In several cases, they are used interchangeably - for example Privacy Notice as a measure or control refers to both the information as well as the act of making it available. For 'active' contexts where this distinction is important, e.g. data breach notifications, see Notification concept."@en .

dpv:NoticeCommunicated a rdfs:Class,
        skos:Concept,
        dpv:NoticeStatus ;
    dct:contributor _:N05cd1f43dbaf4b4ba297dab5ee221394,
        _:N0a43dd9ea5e94fe695d8b7df8802cfdd ;
    dct:created "2024-12-01"^^xsd:date ;
    rdfs:isDefinedBy dpv: ;
    sw:term_status "accepted"@en ;
    skos:broader dpv:NoticeStatus ;
    skos:definition "Status indicating the notice has been communicated"@en ;
    skos:inScheme dpv:notice-classes ;
    skos:prefLabel "Notice Communicated"@en .

dpv:NoticeGenerated a rdfs:Class,
        skos:Concept,
        dpv:NoticeStatus ;
    dct:contributor _:N05cd1f43dbaf4b4ba297dab5ee221394,
        _:N0a43dd9ea5e94fe695d8b7df8802cfdd ;
    dct:created "2024-12-01"^^xsd:date ;
    rdfs:isDefinedBy dpv: ;
    sw:term_status "accepted"@en ;
    skos:broader dpv:NoticeStatus ;
    skos:definition "Status indicating the notice has been generated"@en ;
    skos:inScheme dpv:notice-classes ;
    skos:prefLabel "Notice Generated"@en .

dpv:NoticeIcon a rdfs:Class,
        skos:Concept ;
    dct:created "2024-08-17"^^xsd:date ;
    dct:source [ a schema:WebPage ;
            schema:name "ICO - What methods can we use to provide privacy information?" ;
            schema:url "https://ico.org.uk/for-organisations/uk-gdpr-guidance-and-resources/individual-rights/the-right-to-be-informed/what-methods-can-we-use-to-provide-privacy-information/" ] ;
    vann:example dex:E0072 ;
    rdfs:isDefinedBy dpv: ;
    sw:term_status "accepted"@en ;
    skos:definition "An icon within a notice associated with specific information or elements"@en ;
    skos:inScheme dpv:notice-classes ;
    skos:prefLabel "Notice Icon"@en .

dpv:NoticeLatest a rdfs:Class,
        skos:Concept,
        dpv:NoticeStatus ;
    dct:contributor _:N05cd1f43dbaf4b4ba297dab5ee221394,
        _:N0a43dd9ea5e94fe695d8b7df8802cfdd ;
    dct:created "2024-12-01"^^xsd:date ;
    rdfs:isDefinedBy dpv: ;
    sw:term_status "accepted"@en ;
    skos:broader dpv:NoticeStatus ;
    skos:definition "Status indicating the notice is currently at its latest iteration"@en ;
    skos:inScheme dpv:notice-classes ;
    skos:prefLabel "Notice Latest"@en .

dpv:NoticeLayer a rdfs:Class,
        skos:Concept ;
    dct:created "2024-08-17"^^xsd:date ;
    dct:source [ a schema:WebPage ;
            schema:name "ICO - What methods can we use to provide privacy information?" ;
            schema:url "https://ico.org.uk/for-organisations/uk-gdpr-guidance-and-resources/individual-rights/the-right-to-be-informed/what-methods-can-we-use-to-provide-privacy-information/" ] ;
    vann:example dex:E0072 ;
    rdfs:isDefinedBy dpv: ;
    sw:term_status "accepted"@en ;
    skos:definition "A layer within a layered notice where the layer can be used for providing specific information or controls"@en ;
    skos:inScheme dpv:notice-classes ;
    skos:prefLabel "Notice Layer"@en .

dpv:NoticeStale a rdfs:Class,
        skos:Concept,
        dpv:NoticeStatus ;
    dct:contributor _:N05cd1f43dbaf4b4ba297dab5ee221394,
        _:N0a43dd9ea5e94fe695d8b7df8802cfdd ;
    dct:created "2024-12-01"^^xsd:date ;
    rdfs:isDefinedBy dpv: ;
    sw:term_status "accepted"@en ;
    skos:broader dpv:NoticeStatus ;
    skos:definition "Status indicating the notice is stale or not up to date or not the latest version"@en ;
    skos:inScheme dpv:notice-classes ;
    skos:prefLabel "Notice Stale"@en .

dpv:NoticeStatus a rdfs:Class,
        skos:Concept ;
    dct:contributor _:N05cd1f43dbaf4b4ba297dab5ee221394,
        _:N0a43dd9ea5e94fe695d8b7df8802cfdd ;
    dct:created "2024-12-01"^^xsd:date ;
    vann:example dex:E0073 ;
    rdfs:isDefinedBy dpv: ;
    rdfs:subClassOf dpv:Status ;
    sw:term_status "accepted"@en ;
    skos:broader dpv:Status ;
    skos:definition "Status associated with notice provision, use, and management"@en ;
    skos:inScheme dpv:notice-classes ;
    skos:prefLabel "Notice Status"@en .

dpv:NoticeUnused a rdfs:Class,
        skos:Concept,
        dpv:NoticeStatus ;
    dct:contributor _:N05cd1f43dbaf4b4ba297dab5ee221394,
        _:N0a43dd9ea5e94fe695d8b7df8802cfdd ;
    dct:created "2024-12-01"^^xsd:date ;
    rdfs:isDefinedBy dpv: ;
    sw:term_status "accepted"@en ;
    skos:broader dpv:NoticeStatus ;
    skos:definition "Status indicating the notice has been communicated but has not yet been used e.g. the recipient has not acknowledged it or has not taken the intended action"@en ;
    skos:inScheme dpv:notice-classes ;
    skos:prefLabel "Notice Unused"@en .

dpv:NoticeUpdated a rdfs:Class,
        skos:Concept,
        dpv:NoticeStatus ;
    dct:contributor _:N05cd1f43dbaf4b4ba297dab5ee221394,
        _:N0a43dd9ea5e94fe695d8b7df8802cfdd ;
    dct:created "2024-12-01"^^xsd:date ;
    rdfs:isDefinedBy dpv: ;
    sw:term_status "accepted"@en ;
    skos:broader dpv:NoticeStatus ;
    skos:definition "Status indicating the notice has been updated and its contents or implications have changed"@en ;
    skos:inScheme dpv:notice-classes ;
    skos:prefLabel "Notice Updated"@en .

dpv:NoticeUsed a rdfs:Class,
        skos:Concept,
        dpv:NoticeStatus ;
    dct:contributor _:N05cd1f43dbaf4b4ba297dab5ee221394,
        _:N0a43dd9ea5e94fe695d8b7df8802cfdd ;
    dct:created "2024-12-01"^^xsd:date ;
    rdfs:isDefinedBy dpv: ;
    sw:term_status "accepted"@en ;
    skos:broader dpv:NoticeStatus ;
    skos:definition "Status indicating the notice has been communicated and has been used e.g. the recipient has acknowledged it or taken the intended action"@en ;
    skos:inScheme dpv:notice-classes ;
    skos:prefLabel "Notice Used"@en .

dpv:OralNotice a rdfs:Class,
        skos:Concept,
        dpv:OrganisationalMeasure ;
    dct:created "2024-08-17"^^xsd:date ;
    dct:source [ a schema:WebPage ;
            schema:name "ICO - What methods can we use to provide privacy information?" ;
            schema:url "https://ico.org.uk/for-organisations/uk-gdpr-guidance-and-resources/individual-rights/the-right-to-be-informed/what-methods-can-we-use-to-provide-privacy-information/" ] ;
    rdfs:isDefinedBy dpv: ;
    sw:term_status "accepted"@en ;
    skos:broader dpv:Notice ;
    skos:definition "A notice provided orally or verbally"@en ;
    skos:inScheme dpv:notice-classes ;
    skos:prefLabel "Oral Notice"@en .

dpv:PostedNotice a rdfs:Class,
        skos:Concept,
        dpv:OrganisationalMeasure ;
    dct:created "2024-08-17"^^xsd:date ;
    dct:source [ a schema:WebPage ;
            schema:name "ICO - What methods can we use to provide privacy information?" ;
            schema:url "https://ico.org.uk/for-organisations/uk-gdpr-guidance-and-resources/individual-rights/the-right-to-be-informed/what-methods-can-we-use-to-provide-privacy-information/" ] ;
    rdfs:isDefinedBy dpv: ;
    sw:term_status "accepted"@en ;
    skos:broader dpv:Notice ;
    skos:definition "A notice that is posted as a sign or banner"@en ;
    skos:inScheme dpv:notice-classes ;
    skos:prefLabel "Posted Notice"@en .

dpv:PrintedNotice a rdfs:Class,
        skos:Concept,
        dpv:OrganisationalMeasure ;
    dct:created "2024-08-17"^^xsd:date ;
    dct:source [ a schema:WebPage ;
            schema:name "ICO - What methods can we use to provide privacy information?" ;
            schema:url "https://ico.org.uk/for-organisations/uk-gdpr-guidance-and-resources/individual-rights/the-right-to-be-informed/what-methods-can-we-use-to-provide-privacy-information/" ] ;
    rdfs:isDefinedBy dpv: ;
    sw:term_status "accepted"@en ;
    skos:broader dpv:Notice ;
    skos:definition "A notice that is provided in a printed form on or along with a device"@en ;
    skos:inScheme dpv:notice-classes ;
    skos:prefLabel "Printed Notice"@en .

dpv:PrivacyNotice a rdfs:Class,
        skos:Concept,
        dpv:OrganisationalMeasure ;
    dct:contributor _:N05cd1f43dbaf4b4ba297dab5ee221394,
        _:N0a43dd9ea5e94fe695d8b7df8802cfdd,
        _:N1aa8f48a4f3a40e6a438f71be918d3a1,
        _:Nd0960ac69a57403fb5db2455be10d160 ;
    dct:created "2021-09-08"^^xsd:date ;
    vann:example dex:E0017,
        dex:E0022 ;
    rdfs:isDefinedBy dpv: ;
    sw:term_status "accepted"@en ;
    skos:broader dpv:Notice ;
    skos:definition "Represents a notice or document outlining information regarding privacy"@en ;
    skos:inScheme dpv:notice-classes ;
    skos:prefLabel "Privacy Notice"@en .

dpv:SecurityIncidentNotice a rdfs:Class,
        skos:Concept,
        dpv:OrganisationalMeasure ;
    dct:contributor _:N0a43dd9ea5e94fe695d8b7df8802cfdd ;
    dct:created "2024-04-14"^^xsd:date ;
    rdfs:isDefinedBy dpv: ;
    sw:term_status "accepted"@en ;
    skos:broader dpv:Notice ;
    skos:definition "A notice providing information about security incident(s)"@en ;
    skos:inScheme dpv:notice-classes ;
    skos:prefLabel "Security Incident Notice"@en .

<https://w3id.org/dpv> a owl:Ontology,
        profile:Profile ;
    dct:bibliographicCitation "Harshvardhan J. Pandit, Beatriz Esteves, Georg P. Krog, Paul Ryan, Delaram Golpayegani, Julian Flake (2025) Data Privacy Vocabulary (DPV) – Version 2.0. In: Demartini, G., et al. The Semantic Web – ISWC 2024. ISWC 2024. Lecture Notes in Computer Science, vol 15233. Springer, Cham. https://doi.org/10.1007/978-3-031-77847-6_10" ;
    dct:conformsTo "http://www.w3.org/2000/01/rdf-schema",
        "http://www.w3.org/2004/02/skos/core" ;
    dct:contributor _:N05cd1f43dbaf4b4ba297dab5ee221394,
        _:N0a43dd9ea5e94fe695d8b7df8802cfdd,
        _:N0c29df1c09e34406bfb949a8e7afb527,
        _:N1aa8f48a4f3a40e6a438f71be918d3a1,
        _:N458008bc6195484e9cc557f70eabda31,
        _:Nd0960ac69a57403fb5db2455be10d160 ;
    dct:created "2022-08-18"@en ;
    dct:creator _:N05cd1f43dbaf4b4ba297dab5ee221394,
        _:N0a43dd9ea5e94fe695d8b7df8802cfdd,
        _:N0c29df1c09e34406bfb949a8e7afb527,
        _:N458008bc6195484e9cc557f70eabda31,
        _:Nd0960ac69a57403fb5db2455be10d160,
        [ a dct:Agent,
                foaf:Person ;
            scoro:hasORCID "0000-0002-1208-186X" ;
            org:memberOf [ a foaf:Organization ;
                    foaf:name "ADAPT Centre, Trinity College Dublin" ] ;
            foaf:name "Delaram Golpayegani" ] ;
    dct:description "The Data Privacy Vocabulary (DPV) provides terms (classes and properties) to represent information about processing of personal data, for example - purposes, processing operations, personal data, technical and organisational measures."@en ;
    dct:identifier "https://w3id.org/dpv" ;
    dct:issued "2022-08-18"@en ;
    dct:license <https://www.w3.org/copyright/document-license-2023/> ;
    dct:modified "2025-03-16"@en ;
    dct:publisher <https://www.w3.org/> ;
    dct:source <https://www.w3.org/groups/cg/dpvcg/> ;
    dct:title "Data Privacy Vocabulary (DPV)"@en ;
    bibo:doi "10.5281/zenodo.12505841" ;
    bibo:status "http://purl.org/ontology/bibo/status/published" ;
    vann:preferredNamespacePrefix "dpv" ;
    vann:preferredNamespaceUri "https://w3id.org/dpv#" ;
    rdfs:Label "DPV"@en ;
    owl:versionIRI <https://w3id.org/dpv/2.1> ;
    owl:versionInfo "2.1" ;
    profile:hasResource dpv:serialisation-html,
        dpv:serialisation-jsonld,
        dpv:serialisation-n3,
        dpv:serialisation-rdf,
        dpv:serialisation-ttl,
        <https://w3id.org/dpv/examples>,
        <https://w3id.org/dpv/guides>,
        <https://w3id.org/dpv/primer> ;
    profile:isProfileOf rdfs:,
        skos: ;
    foaf:logo <https://w3id.org/dpv/media/logo.png> ;
    schema:version "2.1" .

dpv:hasNotice a rdf:Property,
        skos:Concept ;
    dcam:rangeIncludes dpv:Notice ;
    dct:contributor _:N05cd1f43dbaf4b4ba297dab5ee221394,
        _:N0a43dd9ea5e94fe695d8b7df8802cfdd,
        _:N0c29df1c09e34406bfb949a8e7afb527,
        _:Nd0960ac69a57403fb5db2455be10d160 ;
    dct:created "2022-06-22"^^xsd:date ;
    rdfs:isDefinedBy dpv: ;
    rdfs:subPropertyOf dpv:hasOrganisationalMeasure ;
    sw:term_status "accepted"@en ;
    skos:broader dpv:hasOrganisationalMeasure ;
    skos:definition "Indicates the use or applicability of a Notice for the specified context"@en ;
    skos:inScheme dpv:notice-properties ;
    skos:prefLabel "has notice"@en ;
    schema:rangeIncludes dpv:Notice .

dpv:hasNoticeIcon a rdf:Property,
        skos:Concept ;
    dcam:rangeIncludes dpv:NoticeIcon ;
    dct:created "2024-08-17"^^xsd:date ;
    vann:example dex:E0072 ;
    rdfs:isDefinedBy dpv: ;
    sw:term_status "accepted"@en ;
    skos:definition "Indicates the concept can be represented graphically using the specified icon"@en ;
    skos:inScheme dpv:notice-properties ;
    skos:prefLabel "has notice icon"@en ;
    schema:rangeIncludes dpv:NoticeIcon .

dpv:hasNoticeLayer a rdf:Property,
        skos:Concept ;
    dcam:domainIncludes dpv:Notice,
        dpv:NoticeLayer ;
    dcam:rangeIncludes dpv:NoticeLayer ;
    dct:created "2024-08-17"^^xsd:date ;
    vann:example dex:E0072 ;
    rdfs:isDefinedBy dpv: ;
    sw:term_status "accepted"@en ;
    skos:definition "Indicates the use of a notice layer within a notice or to associate a layer with another layer"@en ;
    skos:inScheme dpv:notice-properties ;
    skos:prefLabel "has notice layer"@en ;
    schema:domainIncludes dpv:Notice,
        dpv:NoticeLayer ;
    schema:rangeIncludes dpv:NoticeLayer .

dpv:hasNoticeStatus a rdf:Property,
        skos:Concept ;
    dcam:domainIncludes dpv:Notice ;
    dcam:rangeIncludes dpv:NoticeStatus ;
    dct:contributor _:N05cd1f43dbaf4b4ba297dab5ee221394,
        _:N0a43dd9ea5e94fe695d8b7df8802cfdd ;
    dct:created "2024-12-01"^^xsd:date ;
    vann:example dex:E0073 ;
    rdfs:isDefinedBy dpv: ;
    sw:term_status "accepted"@en ;
    skos:definition "Indicates the status of the associated notice"@en ;
    skos:inScheme dpv:notice-properties ;
    skos:prefLabel "has notice status"@en ;
    schema:domainIncludes dpv:Notice ;
    schema:rangeIncludes dpv:NoticeStatus .

dpv:serialisation-html a profile:ResourceDescriptor ;
    dct:conformsTo <https://www.w3.org/TR/html/> ;
    dct:format <https://www.iana.org/assignments/media-types/text/html> ;
    dct:title "Data Privacy Vocabulary (DPV) - HTML serialiation" ;
    profile:hasArtifact <https://w3id.org/dpv/dpv.html> ;
    profile:hasRole role:specification .

dpv:serialisation-jsonld a profile:ResourceDescriptor ;
    dct:conformsTo <https://www.w3.org/TR/json-ld11/> ;
    dct:format <https://www.iana.org/assignments/media-types/application/ld+json> ;
    dct:title "Data Privacy Vocabulary (DPV) - JSON-LD serialiation" ;
    profile:hasArtifact <https://w3id.org/dpv/dpv/dpv.jsonld> ;
    profile:hasRole role:vocabulary .

dpv:serialisation-n3 a profile:ResourceDescriptor ;
    dct:conformsTo <https://www.w3.org/TeamSubmission/n3/> ;
    dct:format <https://www.iana.org/assignments/media-types/text/n3> ;
    dct:title "Data Privacy Vocabulary (DPV) - N3 serialiation" ;
    profile:hasArtifact <https://w3id.org/dpv/dpv/dpv.n3> ;
    profile:hasRole role:vocabulary .

dpv:serialisation-rdf a profile:ResourceDescriptor ;
    dct:conformsTo rdf: ;
    dct:format <https://www.iana.org/assignments/media-types/application/rdf+xml> ;
    dct:title "Data Privacy Vocabulary (DPV) - RDF/XML serialiation" ;
    profile:hasArtifact <https://w3id.org/dpv/dpv/dpv.rdf> ;
    profile:hasRole role:vocabulary .

dpv:serialisation-ttl a profile:ResourceDescriptor ;
    dct:conformsTo <https://www.w3.org/TR/turtle/> ;
    dct:format <https://www.iana.org/assignments/media-types/text/turtle> ;
    dct:title "Data Privacy Vocabulary (DPV) - Turtle serialiation" ;
    profile:hasArtifact <https://w3id.org/dpv/dpv/dpv.ttl> ;
    profile:hasRole role:vocabulary .

<https://w3id.org/dpv/examples> a profile:ResourceDescriptor ;
    dct:conformsTo <https://www.w3.org/TR/html/> ;
    dct:format <https://www.iana.org/assignments/media-types/text/html> ;
    dct:title "Examples for Data Privacy Vocabulary" ;
    profile:hasArtifact <https://w3id.org/dpv/examples> ;
    profile:hasRole role:guidance .

<https://w3id.org/dpv/guides> a profile:ResourceDescriptor ;
    dct:conformsTo <https://www.w3.org/TR/html/> ;
    dct:format <https://www.iana.org/assignments/media-types/text/html> ;
    dct:title "Guides for Data Privacy Vocabulary" ;
    profile:hasArtifact <https://w3id.org/dpv/guides> ;
    profile:hasRole role:guidance .

<https://w3id.org/dpv/primer> a profile:ResourceDescriptor ;
    dct:conformsTo <https://www.w3.org/TR/html/> ;
    dct:format <https://www.iana.org/assignments/media-types/text/html> ;
    dct:title "Primer for Data Privacy Vocabulary" ;
    profile:hasArtifact <https://w3id.org/dpv/primer> ;
    profile:hasRole role:guidance .

dpv:notice-properties a skos:ConceptScheme .

dpv:notice-classes a skos:ConceptScheme .

_:N2bfb2dfcc0b24c5182bd06c242c085fa a foaf:Organization ;
    foaf:name "Signatu AS" .

_:N313d89a6c37147bfac1bbb4aa7f6510b a foaf:Organization ;
    foaf:name "ADAPT Centre, Dublin City University" .

_:N3f64d3533a104953b63bb217ff4665c5 a foaf:Organization ;
    foaf:name "IDLab, IMEC, Ghent University" .

_:N77a9e87e7f0e42959387d0b6a299325f a foaf:Organization ;
    foaf:name "Uniphar PLC" .

_:Nac2d5a6ba12d43d387d630afd6a760ea a foaf:Organization ;
    foaf:name "Dublin City University" .

_:Nd69451d3e8ae4c24b46f61e344aae1e2 a foaf:Organization ;
    foaf:name "University of Koblenz" .

_:N0c29df1c09e34406bfb949a8e7afb527 a dct:Agent,
        foaf:Person ;
    scoro:hasORCID "0009-0006-4623-1463" ;
    org:memberOf _:Nd69451d3e8ae4c24b46f61e344aae1e2 ;
    foaf:name "Julian Flake" .

_:N458008bc6195484e9cc557f70eabda31 a dct:Agent,
        foaf:Person ;
    scoro:hasORCID "0000-0003-0259-7560" ;
    org:memberOf _:N3f64d3533a104953b63bb217ff4665c5 ;
    foaf:name "Beatriz Esteves" .

_:N1aa8f48a4f3a40e6a438f71be918d3a1 a dct:Agent,
        foaf:Person ;
    org:memberOf _:Nac2d5a6ba12d43d387d630afd6a760ea ;
    foaf:name "David Hickey" .

_:Nd0960ac69a57403fb5db2455be10d160 a dct:Agent,
        foaf:Person ;
    scoro:hasORCID "0000-0003-0770-2737" ;
    org:memberOf _:N77a9e87e7f0e42959387d0b6a299325f ;
    foaf:name "Paul Ryan" .

_:N05cd1f43dbaf4b4ba297dab5ee221394 a dct:Agent,
        foaf:Person ;
    org:memberOf _:N2bfb2dfcc0b24c5182bd06c242c085fa ;
    foaf:homepage "https://www.linkedin.com/in/georg-philip-krog-a2a278104/" ;
    foaf:name "Georg P. Krog" .

_:N0a43dd9ea5e94fe695d8b7df8802cfdd a dct:Agent,
        foaf:Person ;
    scoro:hasORCID "0000-0002-5068-3714" ;
    org:memberOf _:N313d89a6c37147bfac1bbb4aa7f6510b ;
    foaf:homepage "https://harshp.com/" ;
    foaf:name "Harshvardhan J. Pandit" .

