@prefix dcat: <http://www.w3.org/ns/dcat#> .
@prefix dct: <http://purl.org/dc/terms/> .
@prefix dex: <https://w3id.org/dpv/examples#> .
@prefix dpv: <https://w3id.org/dpv#> .
@prefix dpvo: <https://w3id.org/dpv/dpv-owl#> .
@prefix foaf: <http://xmlns.com/foaf/0.1/> .
@prefix owl: <http://www.w3.org/2002/07/owl#> .
@prefix rdf: <http://www.w3.org/1999/02/22-rdf-syntax-ns#> .
@prefix rdfs: <http://www.w3.org/2000/01/rdf-schema#> .
@prefix skos: <http://www.w3.org/2004/02/skos/core#> .
@prefix spl: <https://specialprivacy.ercim.eu/langs/usage-policy#> .
@prefix svd: <https://specialprivacy.ercim.eu/vocabs/data#> .
@prefix svpr: <https://specialprivacy.ercim.eu/vocabs/processing#> .
@prefix svpu: <https://specialprivacy.ercim.eu/vocabs/purposes#> .
@prefix sw: <http://www.w3.org/2003/06/sw-vocab-status/ns#> .
@prefix vann: <http://purl.org/vocab/vann/> .
@prefix xsd: <http://www.w3.org/2001/XMLSchema#> .

dct:accessRights a rdf:Property,
        owl:AnnotationProperty ;
    rdfs:label "dct:accessRights"@en ;
    skos:scopeNote "Specfiying constraints on access associated with Rights Exercising (e.g. User must log in) or access to provided data (e.g. access via link)"@en .

dct:format a rdf:Property,
        owl:AnnotationProperty ;
    rdfs:label "dct:format"@en ;
    skos:scopeNote "Specifying the format of provided information, for example a CSV dataset"@en .

dct:hasPart a rdf:Property,
        owl:AnnotationProperty ;
    rdfs:label "dct:hasPart"@en ;
    skos:scopeNote "Specifying a RightExerciseRecord has RightExerciseActivity as part of its records"@en .

dct:isPartOf a rdf:Property,
        owl:AnnotationProperty ;
    rdfs:label "dct:isPartOf"@en ;
    skos:scopeNote "Specifying a RightExerciseActivity is part of a RightExerciseRecord"@en .

dct:valid a rdf:Property,
        owl:AnnotationProperty ;
    rdfs:label "dct:valid"@en ;
    skos:scopeNote "Specfiying the temporal validity of an activity associated with Right Exercise. For example, limits on duration for providing or accessing provided information"@en .

dcat:Resource a owl:Class ;
    rdfs:label "dcat:Resource"@en ;
    skos:scopeNote "A dataset, data service, or any other resource associated with Right Exercise - such as for providing a copy of personal data"@en .

foaf:page a rdf:Property,
        owl:AnnotationProperty ;
    rdfs:label "foaf:page"@en ;
    skos:scopeNote "Indicates a web page or document providing information or functionality associated with a Right Exercise"@en .

dpv:DataController a owl:Class ;
    rdfs:label "dpv:DataController"@en ;
    skos:scopeNote "An Data Controller can be a Data Source, e.g. a Controller inferring data or generating data"@en .

dpv:DataSubject a owl:Class ;
    rdfs:label "dpv:DataSubject"@en ;
    skos:scopeNote "A Data Subject as a Data Source, e.g. when data is collected via a form or observed from their activities"@en .

dpv:ThirdParty a owl:Class ;
    rdfs:label "dpv:ThirdParty"@en ;
    skos:scopeNote "A Third Party can be a Data Source, e.g. when data is collected from an entity that is neither the Controller nor the Data Subject"@en .

dpv:hasJustification a rdf:Property,
        owl:AnnotationProperty ;
    rdfs:label "dpv:hasJustification"@en ;
    skos:scopeNote "Specifying a justification for non-fulfilment of Right Exercise"@en .

dpv:hasRecipient a rdf:Property,
        owl:AnnotationProperty ;
    rdfs:label "dpv:hasRecipient"@en ;
    skos:scopeNote "Indicates the Recipient of a Right Exercise Activity"@en .

dpv:hasStatus a rdf:Property,
        owl:AnnotationProperty ;
    rdfs:label "dpv:hasStatus"@en ;
    skos:scopeNote "Indicates the status of a Right Exercise Activity"@en .

dpv:isAfter a rdf:Property,
        owl:AnnotationProperty ;
    rdfs:label "dpv:isAfter"@en ;
    skos:scopeNote "Specifying a RightExerciseActivity occurs before another RightExerciseActivity"@en .

dpv:isBefore a rdf:Property,
        owl:AnnotationProperty ;
    rdfs:label "dpv:isBefore"@en ;
    skos:scopeNote "Specifying a RightExerciseActivity occurs before another RightExerciseActivity"@en .

dpv:isImplementedByEntity a rdf:Property,
        owl:AnnotationProperty ;
    rdfs:label "dpv:isImplementedByEntity"@en ;
    skos:scopeNote "Indicates the Entity that implements or performs a Right Exercise Activity"@en .

<https://w3id.org/dpv/dpv-owl> a owl:Ontology ;
    dct:abstract "The Data Privacy Vocabulary (DPV) provides terms (classes and properties) to represent information about legally compliant personal data handling, which includes purposes, processing, personal data, technical and organisational measures."@en ;
    dct:contributor "Axel Polleres",
        "Beatriz Esteves",
        "Bert Bos",
        "Bud Bruegger",
        "Elmar Kiesling",
        "Eva Schlehahn",
        "Fajar J. Ekaputra",
        "Georg P Krog",
        "Harshvardhan J. Pandit",
        "Javier D. Fernández",
        "Julian Flake",
        "Mark Lizar",
        "Paul Ryan",
        "Piero Bonatti",
        "Ramisa Gachpaz Hamed",
        "Rigo Wenning",
        "Rob Brennan",
        "Simon Steyskal" ;
    dct:created "2019-06-18"^^xsd:date ;
    dct:creator "Axel Polleres",
        "Harshvardhan J. Pandit" ;
    dct:description "The Data Privacy Vocabulary (DPV) provides terms (classes and properties) to represent information about legally compliant personal data handling, which includes purposes, processing, personal data, technical and organisational measures."@en ;
    dct:license <https://www.w3.org/Consortium/Legal/2015/doc-license> ;
    dct:modified "2022-12-05"^^xsd:date ;
    dct:source <https://www.w3.org/community/dpvcg/> ;
    dct:title "Data Privacy Vocabulary"@en ;
    vann:preferredNamespacePrefix "dpvo" ;
    vann:preferredNamespaceUri "https://w3id.org/dpv/dpv-owl#"^^xsd:string ;
    owl:versionInfo "1"^^xsd:string .

dpvo:AcademicResearch a owl:Class ;
    rdfs:label "Academic Research"@en ;
    dct:created "2019-04-05"^^xsd:date ;
    dct:creator "Axel Polleres"^^xsd:string,
        "Elmar Kiesling"^^xsd:string,
        "Fajar Ekaputra"^^xsd:string,
        "Harshvardhan J. Pandit"^^xsd:string,
        "Javier Fernandez"^^xsd:string,
        "Simon Steyskal"^^xsd:string ;
    dct:description "Purposes associated with conducting or assisting with research conducted in an academic context e.g. within universities"@en ;
    rdfs:isDefinedBy dpvo: ;
    rdfs:seeAlso svpu:Education ;
    rdfs:subClassOf dpvo:ResearchAndDevelopment ;
    sw:term_status "accepted"@en .

dpvo:AcademicScientificOrganisation a owl:Class ;
    rdfs:label "Academic or Scientific Organisation"@en ;
    dct:created "2022-02-02"^^xsd:date ;
    dct:creator "Harshvardhan J. Pandit"^^xsd:string ;
    dct:description "Organisations related to academia or scientific pursuits e.g. Universities, Schools, Research Bodies"@en ;
    dct:modified "2020-10-05"^^xsd:date ;
    dct:source <http://purl.org/adms> ;
    rdfs:isDefinedBy dpvo: ;
    rdfs:subClassOf dpvo:Organisation ;
    sw:term_status "modified"@en .

dpvo:Access a owl:Class ;
    rdfs:label "Access"@en ;
    dct:created "2022-06-15"^^xsd:date ;
    dct:creator "Georg P Krog"^^xsd:string,
        "Harshvardhan J. Pandit"^^xsd:string ;
    dct:description "to access data"@en ;
    rdfs:isDefinedBy dpvo: ;
    rdfs:subClassOf dpvo:Use ;
    sw:term_status "accepted"@en .

dpvo:AccountManagement a owl:Class ;
    rdfs:label "Account Management"@en ;
    dct:created "2021-09-08"^^xsd:date ;
    dct:creator "Beatriz Esteves"^^xsd:string,
        "Georg P Krog"^^xsd:string,
        "Harshvardhan J. Pandit"^^xsd:string ;
    dct:description "Account Management refers to purposes associated with account management, such as to create, provide, maintain, and manage accounts"@en ;
    rdfs:isDefinedBy dpvo: ;
    rdfs:subClassOf dpvo:Purpose ;
    sw:term_status "accepted"@en .

dpvo:Acquire a owl:Class ;
    rdfs:label "Acquire"@en ;
    dct:created "2019-05-07"^^xsd:date ;
    dct:description "to come into possession or control of the data"@en ;
    dct:source <https://eur-lex.europa.eu/eli/reg/2016/679/art_4/par_2/oj> ;
    rdfs:isDefinedBy dpvo: ;
    rdfs:subClassOf dpvo:Obtain ;
    sw:term_status "accepted"@en .

dpvo:ActivityCompleted a owl:NamedIndividual,
        dpvo:ActivityStatus ;
    rdfs:label "Activity Completed"@en ;
    dct:created "2022-05-18"^^xsd:date ;
    dct:creator "Harshvardhan J. Pandit"^^xsd:string ;
    dct:description "State of an activity that has completed i.e. is fully in the past"@en ;
    rdfs:isDefinedBy dpvo: ;
    sw:term_status "accepted"@en .

dpvo:ActivityHalted a owl:NamedIndividual,
        dpvo:ActivityStatus ;
    rdfs:label "Activity Halted"@en ;
    dct:created "2022-05-18"^^xsd:date ;
    dct:creator "Harshvardhan J. Pandit"^^xsd:string ;
    dct:description "State of an activity that was occuring in the past, and has been halted or paused or stoped"@en ;
    rdfs:isDefinedBy dpvo: ;
    sw:term_status "accepted"@en .

dpvo:ActivityMonitoring a owl:Class ;
    rdfs:label "Activity Monitoring"@en ;
    dct:created "2022-08-17"^^xsd:date ;
    dct:creator "Harshvardhan J. Pandit"^^xsd:string ;
    dct:description "Monitoring of activities including assessing whether they have been successfully initiated and completed"@en ;
    dct:source <https://www.enisa.europa.eu/publications/reference-incident-classification-taxonomy/> ;
    rdfs:isDefinedBy dpvo: ;
    rdfs:subClassOf dpvo:TechnicalMeasure ;
    sw:term_status "accepted"@en .

dpvo:ActivityNotCompleted a owl:NamedIndividual,
        dpvo:ActivityStatus ;
    rdfs:label "Acitivity Not Completed"@en ;
    dct:created "2022-11-30"^^xsd:date ;
    dct:creator "Harshvardhan J. Pandit"^^xsd:string ;
    dct:description "State of an activity that could not be completed, but has reached some end state"@en ;
    rdfs:comment "This relates to a 'Stop' state as distinct from a 'Halt' state. It makes no comments on whether the Acitivity can be resumed or continued towards completion."@en ;
    rdfs:isDefinedBy dpvo: ;
    sw:term_status "accepted"@en .

dpvo:ActivityOngoing a owl:NamedIndividual,
        dpvo:ActivityStatus ;
    rdfs:label "Activity Ongoing"@en ;
    dct:created "2022-05-18"^^xsd:date ;
    dct:creator "Harshvardhan J. Pandit"^^xsd:string ;
    dct:description "State of an activity occuring in continuation i.e. currently ongoing"@en ;
    rdfs:isDefinedBy dpvo: ;
    sw:term_status "accepted"@en .

dpvo:ActivityProposed a owl:NamedIndividual,
        dpvo:ActivityStatus ;
    rdfs:label "Activity Proposed"@en ;
    dct:created "2022-05-18"^^xsd:date ;
    dct:creator "Harshvardhan J. Pandit"^^xsd:string ;
    dct:description "State of an activity being proposed or planned i.e. yet to occur"@en ;
    rdfs:isDefinedBy dpvo: ;
    sw:term_status "accepted"@en .

dpvo:Adapt a owl:Class ;
    rdfs:label "Adapt"@en ;
    dct:created "2019-05-07"^^xsd:date ;
    dct:description "to modify the data, often rewritten into a new form for a new use"@en ;
    dct:source <https://eur-lex.europa.eu/eli/reg/2016/679/art_4/par_2/oj> ;
    rdfs:isDefinedBy dpvo: ;
    rdfs:subClassOf dpvo:Transform ;
    sw:term_status "accepted"@en .

dpvo:Adult a owl:Class ;
    rdfs:label "Adult"@en ;
    dct:created "2022-03-30"^^xsd:date ;
    dct:creator "Georg Krog"^^xsd:string ;
    dct:description "A natural person that is not a child i.e. has attained some legally specified age of adulthood"@en ;
    rdfs:isDefinedBy dpvo: ;
    rdfs:subClassOf dpvo:DataSubject ;
    sw:term_status "accepted"@en .

dpvo:Align a owl:Class ;
    rdfs:label "Align"@en ;
    dct:created "2019-05-07"^^xsd:date ;
    dct:description "to adjust the data to be in relation to another data"@en ;
    dct:source <https://eur-lex.europa.eu/eli/reg/2016/679/art_4/par_2/oj> ;
    rdfs:isDefinedBy dpvo: ;
    rdfs:subClassOf dpvo:Transform ;
    sw:term_status "accepted"@en .

dpvo:Analyse a owl:Class ;
    rdfs:label "Analyse"@en ;
    dct:created "2019-05-07"^^xsd:date ;
    dct:description "to study or examine the data in detail"@en ;
    dct:source <https://specialprivacy.ercim.eu/vocabs/processing> ;
    rdfs:isDefinedBy dpvo: ;
    rdfs:seeAlso svpr:Analyse ;
    rdfs:subClassOf dpvo:Use ;
    sw:term_status "accepted"@en .

dpvo:Anonymisation a owl:Class ;
    rdfs:label "Anonymisation"@en ;
    dct:created "2019-04-05"^^xsd:date ;
    dct:creator "Axel Polleres"^^xsd:string,
        "Harshvardhan J. Pandit"^^xsd:string,
        "Mark Lizar"^^xsd:string,
        "Rob Brennan"^^xsd:string ;
    dct:description "Anonymisation is the process by which data is irreversibly altered in such a way that a data subject can no longer be identified directly or indirectly, either by the entity holding the data alone or in collaboration with other entities and information sources"@en ;
    dct:modified "2022-11-24"^^xsd:date ;
    dct:source <https://www.iso.org/standard/45123.html> ;
    rdfs:isDefinedBy dpvo: ;
    rdfs:subClassOf dpvo:Deidentification ;
    sw:term_status "modified"@en .

dpvo:Anonymise a owl:Class ;
    rdfs:label "Anonymise"@en ;
    dct:created "2019-05-07"^^xsd:date ;
    dct:description "to irreversibly alter personal data in such a way that an unique data subject can no longer be identified directly or indirectly or in combination with other data"@en ;
    dct:source <https://specialprivacy.ercim.eu/vocabs/processing> ;
    rdfs:isDefinedBy dpvo: ;
    rdfs:seeAlso svpr:Anonymise ;
    rdfs:subClassOf dpvo:Transform ;
    sw:term_status "accepted"@en .

dpvo:AnonymisedData a owl:Class ;
    rdfs:label "Anonymised Data"@en ;
    dct:created "2022-01-19"^^xsd:date ;
    dct:creator "Piero Bonatti"^^xsd:string ;
    dct:description "Personal Data that has been (fully and completely) anonymised so that it is no longer considered Personal Data"@en ;
    rdfs:comment "It is advised to carefully consider indicating data is fully or completely anonymised by determining whether the data by itself or in combination with other data can identify a person. Failing this condition, the data should be denoted as PseudonymisedData. To indicate data is anonymised only for a specified entity (e.g. within an organisation), the concept ContextuallyAnonymisedData (as subclass of PseudonymisedData) should be used instead of AnonymisedData."@en ;
    rdfs:isDefinedBy dpvo: ;
    rdfs:subClassOf dpvo:NonPersonalData ;
    sw:term_status "accepted"@en .

dpvo:AntiTerrorismOperations a owl:Class ;
    rdfs:label "Anti-Terrorism Operations"@en ;
    dct:created "2022-04-20"^^xsd:date ;
    dct:creator "Harshvardhan J. Pandit"^^xsd:string ;
    dct:description "Purposes associated with activities that detect, prevent, mitigate, or perform other activities for anti-terrorism"@en ;
    rdfs:isDefinedBy dpvo: ;
    rdfs:subClassOf dpvo:EnforceSecurity ;
    sw:term_status "accepted"@en .

dpvo:Assess a owl:Class ;
    rdfs:label "Assess"@en ;
    dct:created "2022-06-15"^^xsd:date ;
    dct:creator "Georg P Krog"^^xsd:string,
        "Harshvardhan J. Pandit"^^xsd:string ;
    dct:description "to assess data for some criteria"@en ;
    rdfs:isDefinedBy dpvo: ;
    rdfs:subClassOf dpvo:Use ;
    sw:term_status "accepted"@en .

dpvo:AssetManagementProcedures a owl:Class ;
    rdfs:label "Asset Management Procedures"@en ;
    dct:created "2022-08-17"^^xsd:date ;
    dct:creator "Harshvardhan J. Pandit"^^xsd:string ;
    dct:description "Procedures related to management of assets"@en ;
    dct:source <https://www.enisa.europa.eu/publications/5g-cybersecurity-standards> ;
    rdfs:isDefinedBy dpvo: ;
    rdfs:subClassOf dpvo:GovernanceProcedures ;
    sw:term_status "accepted"@en .

dpvo:AsylumSeeker a owl:Class ;
    rdfs:label "Asylum Seeker"@en ;
    dct:created "2022-06-15"^^xsd:date ;
    dct:creator "Georg P Krog"^^xsd:string ;
    dct:description "Data subjects that are asylum seekers"@en ;
    rdfs:isDefinedBy dpvo: ;
    rdfs:subClassOf dpvo:VulnerableDataSubject ;
    sw:term_status "accepted"@en .

dpvo:AsymmetricCryptography a owl:Class ;
    rdfs:label "Asymmetric Cryptography"@en ;
    dct:created "2022-08-17"^^xsd:date ;
    dct:creator "Harshvardhan J. Pandit"^^xsd:string ;
    dct:description "Use of public-key cryptography or asymmetric cryptography involving a public and private pair of keys"@en ;
    dct:source <https://www.enisa.europa.eu/publications/reference-incident-classification-taxonomy/> ;
    rdfs:isDefinedBy dpvo: ;
    rdfs:subClassOf dpvo:CryptographicMethods ;
    sw:term_status "accepted"@en .

dpvo:AsymmetricEncryption a owl:Class ;
    rdfs:label "Asymmetric Encryption"@en ;
    dct:created "2022-08-17"^^xsd:date ;
    dct:creator "Harshvardhan J. Pandit"^^xsd:string ;
    dct:description "Use of asymmetric cryptography to encrypt data"@en ;
    dct:source <https://www.enisa.europa.eu/publications/data-pseudonymisation-advanced-techniques-and-use-cases> ;
    rdfs:isDefinedBy dpvo: ;
    rdfs:subClassOf dpvo:Encryption ;
    sw:term_status "accepted"@en .

dpvo:AuditApproved a owl:NamedIndividual,
        dpvo:AuditStatus ;
    rdfs:label "Audit Approved"@en ;
    dct:created "2022-05-18"^^xsd:date ;
    dct:creator "Harshvardhan J. Pandit"^^xsd:string ;
    dct:description "State of being approved through the audit"@en ;
    rdfs:isDefinedBy dpvo: ;
    sw:term_status "accepted"@en .

dpvo:AuditConditionallyApproved a owl:NamedIndividual,
        dpvo:AuditStatus ;
    rdfs:label "Audit Conditionally Approved"@en ;
    dct:created "2022-06-29"^^xsd:date ;
    dct:creator "Paul Ryan"^^xsd:string ;
    dct:description "State of being conditionally approved through the audit"@en ;
    rdfs:comment "A \"conditional approval\" is intended to reflect states where the audit has identified further changes which must be implemented before considering the audit has been 'passed', without requiring another audit to validate them. This is distinct from the case where an audit has state 'rejected', which means changes must be made and submitted for review. The requirements of a 'conditional acceptance' are expected to be minor or not significant enough to warrant another audit to review them."@en ;
    rdfs:isDefinedBy dpvo: ;
    sw:term_status "accepted"@en .

dpvo:AuditNotRequired a owl:NamedIndividual,
        dpvo:AuditStatus ;
    rdfs:label "Audit Not Required"@en ;
    dct:created "2022-05-18"^^xsd:date ;
    dct:creator "Harshvardhan J. Pandit"^^xsd:string ;
    dct:description "State where an audit is determined as not being required"@en ;
    rdfs:isDefinedBy dpvo: ;
    sw:term_status "accepted"@en .

dpvo:AuditRejected a owl:NamedIndividual,
        dpvo:AuditStatus ;
    rdfs:label "Audit Rejected"@en ;
    dct:created "2022-05-18"^^xsd:date ;
    dct:creator "Harshvardhan J. Pandit"^^xsd:string ;
    dct:description "State of not being approved or being rejected through the audit"@en ;
    rdfs:isDefinedBy dpvo: ;
    sw:term_status "accepted"@en .

dpvo:AuditRequested a owl:NamedIndividual,
        dpvo:AuditStatus ;
    rdfs:label "Audit Requested"@en ;
    dct:created "2022-05-18"^^xsd:date ;
    dct:creator "Harshvardhan J. Pandit"^^xsd:string ;
    dct:description "State of an audit being requested whose outcome is not yet known"@en ;
    rdfs:isDefinedBy dpvo: ;
    sw:term_status "accepted"@en .

dpvo:AuditRequired a owl:NamedIndividual,
        dpvo:AuditStatus ;
    rdfs:label "Audit Required"@en ;
    dct:created "2022-05-18"^^xsd:date ;
    dct:creator "Harshvardhan J. Pandit"^^xsd:string ;
    dct:description "State where an audit is determined as being required but has not been conducted"@en ;
    rdfs:isDefinedBy dpvo: ;
    sw:term_status "accepted"@en .

dpvo:Authentication-ABC a owl:Class ;
    rdfs:label "Authentication using ABC"@en ;
    dct:created "2022-08-17"^^xsd:date ;
    dct:creator "Harshvardhan J. Pandit"^^xsd:string ;
    dct:description "Use of Attribute Based Credentials (ABC) to perform and manage authentication"@en ;
    dct:source <https://www.enisa.europa.eu/publications/data-protection-engineering> ;
    rdfs:isDefinedBy dpvo: ;
    rdfs:subClassOf dpvo:CryptographicAuthentication ;
    sw:term_status "accepted"@en .

dpvo:Authentication-PABC a owl:Class ;
    rdfs:label "Authentication using PABC"@en ;
    dct:created "2022-08-17"^^xsd:date ;
    dct:creator "Harshvardhan J. Pandit"^^xsd:string ;
    dct:description "Use of Privacy-enhacing Attribute Based Credentials (ABC) to perform and manage authentication"@en ;
    dct:source <https://www.enisa.europa.eu/publications/data-protection-engineering> ;
    rdfs:isDefinedBy dpvo: ;
    rdfs:subClassOf dpvo:CryptographicAuthentication ;
    sw:term_status "accepted"@en .

dpvo:AuthorisationProtocols a owl:Class ;
    rdfs:label "Authorisation Protocols"@en ;
    dct:created "2022-08-17"^^xsd:date ;
    dct:creator "Harshvardhan J. Pandit"^^xsd:string ;
    dct:description "Protocols involving authorisation of roles or profiles to determine permission, rights, or privileges"@en ;
    dct:source <https://www.enisa.europa.eu/publications/reference-incident-classification-taxonomy/> ;
    rdfs:isDefinedBy dpvo: ;
    rdfs:subClassOf dpvo:TechnicalMeasure ;
    sw:term_status "accepted"@en .

dpvo:AutomatedDecisionMaking a owl:Class ;
    rdfs:label "Automated Decision Making"@en ;
    dct:created "2020-11-04"^^xsd:date ;
    dct:creator "Harshvardhan J. Pandit"^^xsd:string,
        "Piero Bonatti"^^xsd:string ;
    dct:description "Processing that involves automated decision making"@en ;
    dct:modified "2022-09-07"^^xsd:date ;
    dct:source <https://eur-lex.europa.eu/eli/reg/2016/679/art_4/par_2/oj> ;
    rdfs:comment "Automated decision making can be defined as “the ability to make decisions by technological means without human involvement.” (“Guidelines on Automated individual decision-making and Profiling for the purposes of Regulation 2016/679 (wp251rev.01)”, 2018, p. 8)"@en ;
    rdfs:isDefinedBy dpvo: ;
    rdfs:subClassOf dpvo:AutomationOfProcessing,
        dpvo:DecisionMaking ;
    sw:term_status "modified"@en .

dpvo:AutomatedProcessingWithHumanInput a owl:NamedIndividual,
        dpvo:AutomationOfProcessing,
        dpvo:HumanInvolvementForInput ;
    rdfs:label "Automated Processing with Human Input"@en ;
    dct:created "2022-06-15"^^xsd:date ;
    dct:creator "Harshvardhan J. Pandit"^^xsd:string ;
    dct:description "Processing that is automated and involves inputs by Humans"@en ;
    dct:modified "2022-09-07"^^xsd:date ;
    rdfs:comment "For example, an algorithm that takes inputs from humans and performs operations based on them"@en ;
    rdfs:isDefinedBy dpvo: ;
    sw:term_status "accepted"@en .

dpvo:AutomatedProcessingWithHumanOversight a owl:NamedIndividual,
        dpvo:AutomationOfProcessing,
        dpvo:HumanInvolvementForOversight ;
    rdfs:label "Automated Processing with Human Oversight"@en ;
    dct:created "2022-06-15"^^xsd:date ;
    dct:creator "Harshvardhan J. Pandit"^^xsd:string ;
    dct:description "Processing that is automated and involves oversight by Humans"@en ;
    dct:modified "2022-09-07"^^xsd:date ;
    rdfs:comment "For example, a human watching metrics to ensure correctness of procedural values and outputs as processing takes place"@en ;
    rdfs:isDefinedBy dpvo: ;
    sw:term_status "accepted"@en .

dpvo:AutomatedProcessingWithHumanReview a owl:NamedIndividual,
        dpvo:AutomationOfProcessing,
        dpvo:HumanInvolvementForVerification ;
    rdfs:label "Automated Processing with Human Review"@en ;
    dct:created "2022-06-15"^^xsd:date ;
    dct:creator "Harshvardhan J. Pandit"^^xsd:string ;
    dct:description "Processing that is automated and involves review by Humans"@en ;
    dct:modified "2020-10-05"^^xsd:date ;
    rdfs:comment "For example, a human verifying outputs of an algorithm for correctness or impact to individuals"@en ;
    rdfs:isDefinedBy dpvo: ;
    sw:term_status "modified"@en .

dpvo:BackgroundChecks a owl:Class ;
    rdfs:label "Background Checks"@en ;
    dct:created "2022-08-17"^^xsd:date ;
    dct:creator "Harshvardhan J. Pandit"^^xsd:string ;
    dct:description "Procedure where the background of an entity is assessed to identity vulnerabilities and threats due to their current or intended role"@en ;
    dct:source <https://www.enisa.europa.eu/publications/5g-cybersecurity-standards> ;
    rdfs:isDefinedBy dpvo: ;
    rdfs:subClassOf dpvo:SecurityProcedure ;
    sw:term_status "accepted"@en .

dpvo:Benefit a owl:Class ;
    rdfs:label "Benefit"@en ;
    dct:created "2022-03-23"^^xsd:date ;
    dct:creator "Axel Polleres"^^xsd:string,
        "Beatriz Esteves"^^xsd:string,
        "Fajar Ekaputra"^^xsd:string,
        "Georg P Krog"^^xsd:string,
        "Harshvardhan J. Pandit"^^xsd:string,
        "Julian Flake"^^xsd:string ;
    dct:description "Impact(s) that acts as or causes benefits"@en ;
    rdfs:isDefinedBy dpvo: ;
    rdfs:subClassOf dpvo:Impact ;
    sw:term_status "accepted"@en .

dpvo:BiometricAuthentication a owl:Class ;
    rdfs:label "Biometric Authentication"@en ;
    dct:created "2022-08-17"^^xsd:date ;
    dct:creator "Harshvardhan J. Pandit"^^xsd:string ;
    dct:description "Use of biometric data for authentication"@en ;
    dct:source <https://www.enisa.europa.eu/publications/reference-incident-classification-taxonomy/> ;
    rdfs:isDefinedBy dpvo: ;
    rdfs:subClassOf dpvo:AuthenticationProtocols ;
    sw:term_status "accepted"@en .

dpvo:Certification a owl:Class ;
    rdfs:label "Certification"@en ;
    dct:created "2019-04-05"^^xsd:date ;
    dct:creator "Axel Polleres"^^xsd:string,
        "Harshvardhan J. Pandit"^^xsd:string,
        "Mark Lizar"^^xsd:string,
        "Rob Brennan"^^xsd:string ;
    dct:description "Certification mechanisms, seals, and marks for the purpose of demonstrating compliance"@en ;
    rdfs:isDefinedBy dpvo: ;
    rdfs:subClassOf dpvo:CertificationSeal ;
    sw:term_status "accepted"@en .

dpvo:Child a owl:Class ;
    rdfs:label "Child"@en ;
    dct:created "2020-11-25"^^xsd:date ;
    dct:creator "Harshvardhan J. Pandit"^^xsd:string ;
    dct:description "A 'child' is a natural legal person who is below a certain legal age depending on the legal jurisdiction."@en ;
    dct:modified "2022-06-22"^^xsd:date ;
    rdfs:comment "The legality of age defining a child varies by jurisdiction. In addition, 'child' is distinct from a 'minor'. For example, the legal age for consumption of alcohol can be 21, which makes a person of age 20 a 'minor' in this context. In other cases, 'minor' and 'child' are used interchangeably to refer to a person below some legally defined age."@en ;
    rdfs:isDefinedBy dpvo: ;
    rdfs:subClassOf dpvo:DataSubject ;
    sw:term_status "changed"@en .

dpvo:Citizen a owl:Class ;
    rdfs:label "Citizen"@en ;
    dct:created "2022-04-06"^^xsd:date ;
    dct:creator "Beatriz Esteves"^^xsd:string,
        "Georg P. Krog"^^xsd:string,
        "Harshvardhan J. Pandit"^^xsd:string,
        "Julian Flake"^^xsd:string,
        "Paul Ryan"^^xsd:string ;
    dct:description "Data subjects that are citizens (for a jurisdiction)"@en ;
    rdfs:isDefinedBy dpvo: ;
    rdfs:subClassOf dpvo:DataSubject ;
    sw:term_status "accepted"@en .

dpvo:City a owl:Class ;
    rdfs:label "City"@en ;
    dct:created "2022-10-22"^^xsd:date ;
    dct:creator "Harshvardhan J. Pandit"^^xsd:string ;
    dct:description "A region consisting of urban population and commerce"@en ;
    rdfs:isDefinedBy dpvo: ;
    rdfs:subClassOf dpvo:Location ;
    sw:term_status "accepted"@en .

dpvo:Client a owl:Class ;
    rdfs:label "Client"@en ;
    dct:created "2022-04-06"^^xsd:date ;
    dct:creator "Beatriz Esteves"^^xsd:string,
        "Georg P. Krog"^^xsd:string,
        "Harshvardhan J. Pandit"^^xsd:string,
        "Julian Flake"^^xsd:string,
        "Paul Ryan"^^xsd:string ;
    dct:description "Data subjects that are clients or recipients of services"@en ;
    rdfs:isDefinedBy dpvo: ;
    rdfs:subClassOf dpvo:Customer ;
    sw:term_status "accepted"@en .

dpvo:CloudLocation a owl:Class ;
    rdfs:label "Cloud Location"@en ;
    dct:created "2022-06-15"^^xsd:date ;
    dct:creator "Harshvardhan J. Pandit"^^xsd:string ;
    dct:description "Location that is in the 'cloud' i.e. a logical location operated over the internet"@en ;
    dct:modified "2020-10-05"^^xsd:date ;
    rdfs:isDefinedBy dpvo: ;
    rdfs:subClassOf dpvo:RemoteLocation ;
    sw:term_status "modified"@en .

dpvo:CodeOfConduct a owl:Class ;
    rdfs:label "Code of Conduct"@en ;
    dct:created "2019-04-05"^^xsd:date ;
    dct:creator "Axel Polleres"^^xsd:string,
        "Harshvardhan J. Pandit"^^xsd:string,
        "Mark Lizar"^^xsd:string,
        "Rob Brennan"^^xsd:string ;
    dct:description "A set of rules or procedures outlining the norms and practices for conducting activities"@en ;
    rdfs:isDefinedBy dpvo: ;
    rdfs:subClassOf dpvo:GuidelinesPrinciple ;
    sw:term_status "accepted"@en .

dpvo:Collect a owl:Class ;
    rdfs:label "Collect"@en ;
    dct:created "2019-05-07"^^xsd:date ;
    dct:description "to gather data from someone"@en ;
    dct:source <https://eur-lex.europa.eu/eli/reg/2016/679/art_4/par_2/oj>,
        <https://specialprivacy.ercim.eu/vocabs/processing> ;
    rdfs:isDefinedBy dpvo: ;
    rdfs:seeAlso svpr:Collect ;
    rdfs:subClassOf dpvo:Obtain ;
    sw:term_status "accepted"@en .

dpvo:Combine a owl:Class ;
    rdfs:label "Combine"@en ;
    dct:created "2019-05-07"^^xsd:date ;
    dct:description "to join or merge data"@en ;
    dct:source <https://eur-lex.europa.eu/eli/reg/2016/679/art_4/par_2/oj>,
        <https://specialprivacy.ercim.eu/vocabs/processing> ;
    rdfs:isDefinedBy dpvo: ;
    rdfs:seeAlso svpr:Aggregate ;
    rdfs:subClassOf dpvo:Transform ;
    sw:term_status "accepted"@en .

dpvo:CommercialResearch a owl:Class ;
    rdfs:label "Commercial Research"@en ;
    dct:created "2019-04-05"^^xsd:date ;
    dct:creator "Axel Polleres"^^xsd:string,
        "Elmar Kiesling"^^xsd:string,
        "Fajar Ekaputra"^^xsd:string,
        "Harshvardhan J. Pandit"^^xsd:string,
        "Javier Fernandez"^^xsd:string,
        "Simon Steyskal"^^xsd:string ;
    dct:description "Purposes associated with conducting research in a commercial setting or with intention to commercialise e.g. in a company or sponsored by a company"@en ;
    rdfs:isDefinedBy dpvo: ;
    rdfs:seeAlso svpu:Develop ;
    rdfs:subClassOf dpvo:ResearchAndDevelopment ;
    sw:term_status "accepted"@en .

dpvo:CommunicationForCustomerCare a owl:Class ;
    rdfs:label "Communication for Customer Care"@en ;
    dct:created "2020-11-04"^^xsd:date ;
    dct:creator "Beatriz Esteves"^^xsd:string,
        "Georg P Krog"^^xsd:string,
        "Harshvardhan J. Pandit"^^xsd:string ;
    dct:description "Customer Care Communication refers to purposes associated with communicating with customers for assisting them, resolving issues, ensuring satisfaction, etc. in relation to services provided"@en ;
    rdfs:isDefinedBy dpvo: ;
    rdfs:subClassOf dpvo:CommunicationManagement,
        dpvo:CustomerCare ;
    sw:term_status "accepted"@en .

dpvo:CompletelyManualProcessing a owl:NamedIndividual,
        dpvo:AutomationOfProcessing ;
    rdfs:label "Completely Manual Processing"@en ;
    dct:created "2022-06-15"^^xsd:date ;
    dct:creator "Harshvardhan J. Pandit"^^xsd:string ;
    dct:description "Processing that is completely un-automated or fully manual"@en ;
    rdfs:comment "For example, a human performing some processing operation"@en ;
    rdfs:isDefinedBy dpvo: ;
    sw:term_status "accepted"@en .

dpvo:ComplianceIndeterminate a owl:NamedIndividual,
        dpvo:ComplianceStatus ;
    rdfs:label "Compliance Indeterminate"@en ;
    dct:created "2022-09-07"^^xsd:date ;
    dct:creator "Harshvardhan J. Pandit"^^xsd:string ;
    dct:description "State where the status of compliance has not been fully assessed, evaluated, or determined"@en ;
    rdfs:isDefinedBy dpvo: ;
    sw:term_status "accepted"@en .

dpvo:ComplianceMonitoring a owl:Class ;
    rdfs:label "Compliance Monitoring"@en ;
    dct:created "2022-08-17"^^xsd:date ;
    dct:creator "Harshvardhan J. Pandit"^^xsd:string ;
    dct:description "Monitoring of compliance (e.g. internal policy, regulations)"@en ;
    dct:source <https://www.enisa.europa.eu/publications/5g-cybersecurity-standards> ;
    rdfs:isDefinedBy dpvo: ;
    rdfs:subClassOf dpvo:GovernanceProcedures ;
    sw:term_status "accepted"@en .

dpvo:ComplianceUnknown a owl:NamedIndividual,
        dpvo:ComplianceStatus ;
    rdfs:label "Compliance Unknown"@en ;
    dct:created "2022-09-07"^^xsd:date ;
    dct:creator "Harshvardhan J. Pandit"^^xsd:string ;
    dct:description "State where the status of compliance is unknown"@en ;
    rdfs:isDefinedBy dpvo: ;
    sw:term_status "accepted"@en .

dpvo:ComplianceViolation a owl:NamedIndividual,
        dpvo:ComplianceStatus ;
    rdfs:label "Compliance Violation"@en ;
    dct:created "2022-05-18"^^xsd:date ;
    dct:creator "Harshvardhan J. Pandit"^^xsd:string ;
    dct:description "State where compliance cannot be achieved due to requirements being violated"@en ;
    dct:modified "2022-09-07"^^xsd:date ;
    rdfs:comment "Changed from \"violation of compliance\" for consistency with other terms"@en ;
    rdfs:isDefinedBy dpvo: ;
    sw:term_status "changed"@en .

dpvo:Compliant a owl:NamedIndividual,
        dpvo:ComplianceStatus ;
    rdfs:label "Compliant"@en ;
    dct:created "2022-05-18"^^xsd:date ;
    dct:creator "Harshvardhan J. Pandit"^^xsd:string ;
    dct:description "State of being fully compliant"@en ;
    rdfs:isDefinedBy dpvo: ;
    sw:term_status "accepted"@en .

dpvo:Conformant a owl:NamedIndividual,
        dpvo:ConformanceStatus ;
    rdfs:label "Conformant"@en ;
    dct:created "2022-10-22"^^xsd:date ;
    dct:creator "Harshvardhan J. Pandit"^^xsd:string ;
    dct:description "State of being conformant"@en ;
    rdfs:isDefinedBy dpvo: ;
    sw:term_status "accepted"@en .

dpvo:ConsentExpired a owl:NamedIndividual,
        dpvo:ConsentStatusInvalidForProcessing ;
    rdfs:label "Consent Expired"@en ;
    dct:created "2022-06-22"^^xsd:date ;
    dct:creator "Georg P Krog"^^xsd:string,
        "Harshvardhan J. Pandit"^^xsd:string,
        "Julian Flake"^^xsd:string,
        "Paul Ryan"^^xsd:string ;
    dct:description "The state where the temporal or contextual validity of consent has 'expired'"@en ;
    dct:source <https://w3id.org/GConsent> ;
    rdfs:comment "An example of this state is when the obtained consent has been assigned a duration - which has lapsed or 'expired', making it invalid to be used further for processing data"@en ;
    rdfs:isDefinedBy dpvo: ;
    sw:term_status "accepted"@en .

dpvo:ConsentGiven a owl:NamedIndividual,
        dpvo:ConsentStatusValidForProcessing ;
    rdfs:label "Consent Given"@en ;
    dct:created "2022-06-22"^^xsd:date ;
    dct:creator "Georg P Krog"^^xsd:string,
        "Harshvardhan J. Pandit"^^xsd:string,
        "Julian Flake"^^xsd:string,
        "Paul Ryan"^^xsd:string ;
    dct:description "The state where consent has been given"@en ;
    dct:source <https://w3id.org/GConsent> ;
    rdfs:comment "An example of this state is when the individual clicks on a button, ticks a checkbox, verbally agrees - or any other form that communicates their decision agreeing to the processing of data"@en ;
    rdfs:isDefinedBy dpvo: ;
    sw:term_status "accepted"@en .

dpvo:ConsentInvalidated a owl:NamedIndividual,
        dpvo:ConsentStatusInvalidForProcessing ;
    rdfs:label "Consent Invalidated"@en ;
    dct:created "2022-06-22"^^xsd:date ;
    dct:creator "Georg P Krog"^^xsd:string,
        "Harshvardhan J. Pandit"^^xsd:string,
        "Julian Flake"^^xsd:string,
        "Paul Ryan"^^xsd:string ;
    dct:description "The state where consent has been deemed to be invalid"@en ;
    dct:source <https://w3id.org/GConsent> ;
    rdfs:comment "An example of this state is where an investigating authority or a court finds the collected consent did not meet requirements, and 'invalidates' both prior and future uses of it to carry out processing"@en ;
    rdfs:isDefinedBy dpvo: ;
    sw:term_status "accepted"@en .

dpvo:ConsentNotice a owl:Class ;
    rdfs:label "Consent Notice"@en ;
    dct:created "2022-06-21"^^xsd:date ;
    dct:creator "Georg P Krog"^^xsd:string,
        "Harshvardhan J. Pandit"^^xsd:string,
        "Julian Flake"^^xsd:string,
        "Paul Ryan"^^xsd:string ;
    dct:description "A Notice for information provision associated with Consent"@en ;
    rdfs:isDefinedBy dpvo: ;
    rdfs:subClassOf dpvo:PrivacyNotice ;
    sw:term_status "accepted"@en .

dpvo:ConsentRecord a owl:Class ;
    rdfs:label "Consent Record"@en ;
    dct:created "2022-06-22"^^xsd:date ;
    dct:creator "Georg P Krog"^^xsd:string,
        "Harshvardhan J. Pandit"^^xsd:string,
        "Julian Flake"^^xsd:string,
        "Paul Ryan"^^xsd:string ;
    dct:description "A Record of Consent or Consent related activities"@en ;
    rdfs:isDefinedBy dpvo: ;
    rdfs:subClassOf dpvo:DataProcessingRecord ;
    sw:term_status "accepted"@en .

dpvo:ConsentRefused a owl:NamedIndividual,
        dpvo:ConsentStatusInvalidForProcessing ;
    rdfs:label "Consent Refused"@en ;
    dct:created "2022-06-22"^^xsd:date ;
    dct:creator "Georg P Krog"^^xsd:string,
        "Harshvardhan J. Pandit"^^xsd:string,
        "Julian Flake"^^xsd:string,
        "Paul Ryan"^^xsd:string ;
    dct:description "The state where consent has been refused"@en ;
    dct:source <https://w3id.org/GConsent> ;
    rdfs:comment "An example of this state is when the individual clicks on a 'disagree' or 'reject' or 'refuse' button, or leaves a checkbox unticked"@en ;
    rdfs:isDefinedBy dpvo: ;
    sw:term_status "accepted"@en .

dpvo:ConsentRequestDeferred a owl:NamedIndividual,
        dpvo:ConsentStatusInvalidForProcessing ;
    rdfs:label "Consent Request Deferred"@en ;
    dct:created "2022-06-22"^^xsd:date ;
    dct:creator "Georg P Krog"^^xsd:string,
        "Harshvardhan J. Pandit"^^xsd:string,
        "Julian Flake"^^xsd:string,
        "Paul Ryan"^^xsd:string ;
    dct:description "State where a request for consent has been deferred without a decision"@en ;
    dct:source <https://w3id.org/GConsent> ;
    rdfs:comment "An example of this state is when the individual closes or dismisses a notice without making a decision. This state is intended for making the distinction between a notice being provided (as a consent request) and the individual interacting with the notice without making a decision - where the 'ignoring of a notice' is taken as consent being neither given nor refused"@en ;
    rdfs:isDefinedBy dpvo: ;
    sw:term_status "accepted"@en .

dpvo:ConsentRequested a owl:NamedIndividual,
        dpvo:ConsentStatusInvalidForProcessing ;
    rdfs:label "Consent Requested"@en ;
    dct:created "2022-06-22"^^xsd:date ;
    dct:creator "Georg P Krog"^^xsd:string,
        "Harshvardhan J. Pandit"^^xsd:string,
        "Julian Flake"^^xsd:string,
        "Paul Ryan"^^xsd:string ;
    dct:description "State where a request for consent has been made and is awaiting a decision"@en ;
    dct:source <https://w3id.org/GConsent> ;
    rdfs:comment "An example of this state is when a notice has been presented to the individual but they have not made a decision"@en ;
    rdfs:isDefinedBy dpvo: ;
    sw:term_status "accepted"@en .

dpvo:ConsentRevoked a owl:NamedIndividual,
        dpvo:ConsentStatusInvalidForProcessing ;
    rdfs:label "Consent Revoked"@en ;
    dct:created "2022-06-22"^^xsd:date ;
    dct:creator "Georg P Krog"^^xsd:string,
        "Harshvardhan J. Pandit"^^xsd:string,
        "Julian Flake"^^xsd:string,
        "Paul Ryan"^^xsd:string ;
    dct:description "The state where the consent is revoked by an entity other than the data subject and which prevents it from being further used as a valid state"@en ;
    dct:source <https://w3id.org/GConsent> ;
    rdfs:comment "An example of this state is when a Data Controller stops utilising previously obtaining consent, such as when that service no longer exists"@en ;
    rdfs:isDefinedBy dpvo: ;
    sw:term_status "accepted"@en .

dpvo:ConsentUnknown a owl:NamedIndividual,
        dpvo:ConsentStatusInvalidForProcessing ;
    rdfs:label "Consent Unknown"@en ;
    dct:created "2022-06-22"^^xsd:date ;
    dct:creator "Georg P Krog"^^xsd:string,
        "Harshvardhan J. Pandit"^^xsd:string,
        "Julian Flake"^^xsd:string,
        "Paul Ryan"^^xsd:string ;
    dct:description "State where information about consent is not available or is unknown"@en ;
    dct:source <https://w3id.org/GConsent> ;
    rdfs:comment "Consent states can be unknown, for example, when information is not available, or cannot be trusted, or is known to be inaccurate"@en ;
    rdfs:isDefinedBy dpvo: ;
    sw:term_status "accepted"@en .

dpvo:ConsentWithdrawn a owl:NamedIndividual,
        dpvo:ConsentStatusInvalidForProcessing ;
    rdfs:label "Consent Withdrawn"@en ;
    dct:created "2022-06-22"^^xsd:date ;
    dct:creator "Georg P Krog"^^xsd:string,
        "Harshvardhan J. Pandit"^^xsd:string,
        "Julian Flake"^^xsd:string,
        "Paul Ryan"^^xsd:string ;
    dct:description "The state where the consent is withdrawn or revoked specifically by the data subject and which prevents it from being further used as a valid state"@en ;
    dct:source <https://w3id.org/GConsent> ;
    rdfs:comment "This state can be considered a form of 'revocation' of consent, where the revocation can only be performed by the data subject. Therefore we suggest using ConsentRevoked when it is a non-data-subject entity, and ConsentWithdrawn when it is the data subject"@en ;
    rdfs:isDefinedBy dpvo: ;
    sw:term_status "accepted"@en .

dpvo:ConsequenceAsSideEffect a owl:Class ;
    rdfs:label "Consequence as Side-Effect"@en ;
    dct:created "2022-03-30"^^xsd:date ;
    dct:creator "Harshvardhan J. Pandit"^^xsd:string ;
    dct:description "The consequence(s) possible or arising as a side-effect of specified context"@en ;
    rdfs:isDefinedBy dpvo: ;
    rdfs:subClassOf dpvo:Consequence ;
    sw:term_status "accepted"@en .

dpvo:ConsequenceOfFailure a owl:Class ;
    rdfs:label "Consequence of Failure"@en ;
    dct:created "2022-03-23"^^xsd:date ;
    dct:creator "Georg P Krog"^^xsd:string,
        "Harshvardhan J. Pandit"^^xsd:string ;
    dct:description "The consequence(s) possible or arising from failure of specified context"@en ;
    rdfs:isDefinedBy dpvo: ;
    rdfs:subClassOf dpvo:Consequence ;
    sw:term_status "accepted"@en .

dpvo:ConsequenceOfSuccess a owl:Class ;
    rdfs:label "Consequence of Success"@en ;
    dct:created "2022-03-23"^^xsd:date ;
    dct:creator "Georg P Krog"^^xsd:string,
        "Harshvardhan J. Pandit"^^xsd:string ;
    dct:description "The consequence(s) possible or arising from success of specified context"@en ;
    rdfs:isDefinedBy dpvo: ;
    rdfs:subClassOf dpvo:Consequence ;
    sw:term_status "accepted"@en .

dpvo:ConsultationWithAuthority a owl:Class ;
    rdfs:label "Consultation with Authority"@en ;
    dct:created "2020-11-04"^^xsd:date ;
    dct:creator "Georg P Krog"^^xsd:string,
        "Harshvardhan J. Pandit"^^xsd:string,
        "Paul Ryan"^^xsd:string ;
    dct:description "Consultation with an authority or authoritative entity"@en ;
    rdfs:isDefinedBy dpvo: ;
    rdfs:subClassOf dpvo:Consultation ;
    sw:term_status "accepted"@en .

dpvo:ConsultationWithDPO a owl:Class ;
    rdfs:label "Consultation with DPO"@en ;
    dct:created "2022-06-15"^^xsd:date ;
    dct:creator "Georg P Krog"^^xsd:string,
        "Harshvardhan J. Pandit"^^xsd:string ;
    dct:description "Consultation with Data Protection Officer(s)"@en ;
    rdfs:isDefinedBy dpvo: ;
    rdfs:subClassOf dpvo:Consultation ;
    sw:term_status "accepted"@en .

dpvo:ConsultationWithDataSubjectRepresentative a owl:Class ;
    rdfs:label "Consultation with Data Subject Representative"@en ;
    dct:created "2022-10-22"^^xsd:date ;
    dct:creator "Georg P Krog"^^xsd:string,
        "Harshvardhan J. Pandit"^^xsd:string ;
    dct:description "Consultation with representative of data subject(s)"@en ;
    rdfs:isDefinedBy dpvo: ;
    rdfs:subClassOf dpvo:ConsultationWithDataSubject ;
    sw:term_status "accepted"@en .

dpvo:Consumer a owl:Class ;
    rdfs:label "Consumer"@en ;
    dct:created "2022-04-06"^^xsd:date ;
    dct:creator "Beatriz Esteves"^^xsd:string,
        "Georg P. Krog"^^xsd:string,
        "Harshvardhan J. Pandit"^^xsd:string,
        "Julian Flake"^^xsd:string,
        "Paul Ryan"^^xsd:string ;
    dct:description "Data subjects that consume goods or services for direct use"@en ;
    rdfs:isDefinedBy dpvo: ;
    rdfs:subClassOf dpvo:DataSubject ;
    sw:term_status "accepted"@en .

dpvo:ContinousFrequency a owl:Class ;
    rdfs:label "Continous Frequency"@en ;
    dct:created "2022-06-15"^^xsd:date ;
    dct:creator "Harshvardhan J. Pandit"^^xsd:string ;
    dct:description "Frequency where occurences are continous"@en ;
    dct:modified "2020-10-05"^^xsd:date ;
    rdfs:isDefinedBy dpvo: ;
    rdfs:subClassOf dpvo:Frequency ;
    sw:term_status "modified"@en .

dpvo:ContractPerformance a owl:Class ;
    rdfs:label "Contract Performance"@en ;
    dct:created "2021-04-07"^^xsd:date ;
    dct:creator "Georg P Krog"^^xsd:string,
        "Harshvardhan J. Pandit"^^xsd:string,
        "Paul Ryan"^^xsd:string ;
    dct:description "Fulfilment or performance of a contract involving specified processing"@en ;
    rdfs:isDefinedBy dpvo: ;
    rdfs:subClassOf dpvo:Contract ;
    sw:term_status "accepted"@en .

dpvo:ContractualTerms a owl:Class ;
    rdfs:label "Contractual Terms"@en ;
    dct:created "2019-04-05"^^xsd:date ;
    dct:creator "Axel Polleres"^^xsd:string,
        "Harshvardhan J. Pandit"^^xsd:string,
        "Mark Lizar"^^xsd:string,
        "Rob Brennan"^^xsd:string ;
    dct:description "Contractual terms governing data handling within or with an entity"@en ;
    rdfs:isDefinedBy dpvo: ;
    rdfs:subClassOf dpvo:LegalAgreement ;
    sw:term_status "accepted"@en .

dpvo:ControllerProcessorAgreement a owl:Class ;
    rdfs:label "Controller-Processor Agreement"@en ;
    dct:created "2022-01-26"^^xsd:date ;
    dct:creator "Beatriz Esteves"^^xsd:string,
        "Georg P Krog"^^xsd:string,
        "Harshvardhan J. Pandit"^^xsd:string,
        "Julian Flake"^^xsd:string,
        "Paul Ryan"^^xsd:string ;
    dct:description "An agreement outlining conditions, criteria, obligations, responsibilities, and specifics for carrying out processing of personal data between a Data Controller and a Data Processor"@en ;
    rdfs:isDefinedBy dpvo: ;
    rdfs:subClassOf dpvo:DataProcessingAgreement ;
    sw:term_status "accepted"@en .

dpvo:Copy a owl:Class ;
    rdfs:label "Copy"@en ;
    dct:created "2019-05-07"^^xsd:date ;
    dct:description "to produce an exact reprodution of the data"@en ;
    dct:source <https://specialprivacy.ercim.eu/vocabs/processing> ;
    rdfs:isDefinedBy dpvo: ;
    rdfs:seeAlso svpr:Copy ;
    rdfs:subClassOf dpvo:Processing ;
    sw:term_status "accepted"@en .

dpvo:CounterMoneyLaundering a owl:Class ;
    rdfs:label "Counter Money Laundering"@en ;
    dct:created "2022-04-20"^^xsd:date ;
    dct:creator "Harshvardhan J. Pandit"^^xsd:string ;
    dct:description "Purposes associated with detection, prevention, and mitigation of mitigate money laundering"@en ;
    rdfs:isDefinedBy dpvo: ;
    rdfs:subClassOf dpvo:FraudPreventionAndDetection ;
    sw:term_status "accepted"@en .

dpvo:CredentialManagement a owl:Class ;
    rdfs:label "Credential Management"@en ;
    dct:created "2022-06-15"^^xsd:date ;
    dct:creator "Georg P Krog"^^xsd:string ;
    dct:description "Management of credentials and their use in authorisations"@en ;
    rdfs:isDefinedBy dpvo: ;
    rdfs:subClassOf dpvo:AuthorisationProcedure ;
    sw:term_status "accepted"@en .

dpvo:CryptographicKeyManagement a owl:Class ;
    rdfs:label "Cryptographic Key Management"@en ;
    dct:created "2022-08-17"^^xsd:date ;
    dct:creator "Harshvardhan J. Pandit"^^xsd:string ;
    dct:description "Management of cryptographic keys, including their generation, storage, assessment, and safekeeping"@en ;
    dct:source <https://www.enisa.europa.eu/publications/reference-incident-classification-taxonomy/> ;
    rdfs:isDefinedBy dpvo: ;
    rdfs:subClassOf dpvo:CryptographicMethods ;
    sw:term_status "accepted"@en .

dpvo:CustomerClaimsManagement a owl:Class ;
    rdfs:label "Customer Claims Management"@en ;
    dct:created "2021-09-08"^^xsd:date ;
    dct:creator "Beatriz"^^xsd:string,
        "Georg P Krog"^^xsd:string,
        "Harshvardhan J. Pandit"^^xsd:string ;
    dct:description "Customer Claims Management refers to purposes associated with managing claims, including repayment of monies owed"@en ;
    dct:source <https://www.privacycommission.be/nl/model-voor-een-register-van-de-verwerkingsactiviteiten> ;
    rdfs:isDefinedBy dpvo: ;
    rdfs:subClassOf dpvo:CustomerManagement ;
    sw:term_status "accepted"@en .

dpvo:CustomerOrderManagement a owl:Class ;
    rdfs:label "Customer Order Management"@en ;
    dct:created "2021-09-08"^^xsd:date ;
    dct:creator "Beatriz"^^xsd:string,
        "Georg P Krog"^^xsd:string,
        "Harshvardhan J. Pandit"^^xsd:string ;
    dct:description "Customer Order Management refers to purposes associated with managing customer orders i.e. processing of an order related to customer's purchase of good or services"@en ;
    dct:source <https://www.privacycommission.be/nl/model-voor-een-register-van-de-verwerkingsactiviteiten> ;
    rdfs:isDefinedBy dpvo: ;
    rdfs:subClassOf dpvo:CustomerManagement ;
    sw:term_status "accepted"@en .

dpvo:CybersecurityAssessment a owl:Class ;
    rdfs:label "Cybersecurity Assessment"@en ;
    dct:created "2022-08-17"^^xsd:date ;
    dct:creator "Harshvardhan J. Pandit"^^xsd:string ;
    dct:description "Assessment of cybersecurity capabilities in terms of vulnerabilities and effectiveness of controls"@en ;
    dct:source <https://www.enisa.europa.eu/publications/5g-cybersecurity-standards> ;
    rdfs:isDefinedBy dpvo: ;
    rdfs:subClassOf dpvo:Assessment,
        dpvo:SecurityAssessment ;
    sw:term_status "accepted"@en .

dpvo:CybersecurityTraining a owl:Class ;
    rdfs:label "Cybersecurity Training"@en ;
    dct:created "2022-08-17"^^xsd:date ;
    dct:creator "Harshvardhan J. Pandit"^^xsd:string ;
    dct:description "Training methods related to cybersecurity"@en ;
    dct:source <https://www.enisa.europa.eu/publications/reference-incident-classification-taxonomy/> ;
    rdfs:isDefinedBy dpvo: ;
    rdfs:subClassOf dpvo:StaffTraining ;
    sw:term_status "accepted"@en .

dpvo:DPIA a owl:Class ;
    rdfs:label "Data Protection Impact Assessment (DPIA)"@en ;
    dct:created "2020-11-04"^^xsd:date ;
    dct:creator "Georg P Krog"^^xsd:string,
        "Harshvardhan J. Pandit"^^xsd:string,
        "Paul Ryan"^^xsd:string ;
    dct:description "A DPIA involves determining the potential and actual impact of processing activities on individuals or groups of individuals"@en ;
    rdfs:comment "Top class: Impact Assessment, and DPIA is sub-class"@en ;
    rdfs:isDefinedBy dpvo: ;
    rdfs:subClassOf dpvo:ImpactAssessment ;
    sw:term_status "accepted"@en .

dpvo:DataBackupProtocols a owl:Class ;
    rdfs:label "Data Backup Protocols"@en ;
    dct:created "2022-06-15"^^xsd:date ;
    dct:creator "Georg P Krog"^^xsd:string ;
    dct:description "Protocols or plans for backing up of data"@en ;
    rdfs:isDefinedBy dpvo: ;
    rdfs:subClassOf dpvo:TechnicalMeasure ;
    sw:term_status "accepted"@en .

dpvo:DataProtectionAuthority a owl:Class ;
    rdfs:label "Data Protection Authority"@en ;
    dct:created "2020-11-04"^^xsd:date ;
    dct:creator "Georg Krog"^^xsd:string,
        "Harshvardhan Pandit"^^xsd:string,
        "Paul Ryan"^^xsd:string ;
    dct:description "An authority tasked with overseeing legal compliance regarding privacy and data protection laws."@en ;
    rdfs:isDefinedBy dpvo: ;
    rdfs:subClassOf dpvo:Authority ;
    sw:term_status "accepted"@en .

dpvo:DataProtectionTraining a owl:Class ;
    rdfs:label "Data Protection Training"@en ;
    dct:created "2022-08-17"^^xsd:date ;
    dct:creator "Harshvardhan J. Pandit"^^xsd:string ;
    dct:description "Training intended to increase knowledge regarding data protection"@en ;
    dct:source <https://www.enisa.europa.eu/publications/5g-cybersecurity-standards> ;
    rdfs:isDefinedBy dpvo: ;
    rdfs:subClassOf dpvo:StaffTraining ;
    sw:term_status "accepted"@en .

dpvo:DataPublishedByDataSubject a owl:NamedIndividual,
        dpvo:DataSource ;
    rdfs:label "Data published by Data Subject"@en ;
    dct:created "2022-08-24"^^xsd:date ;
    dct:creator "Julian Flake"^^xsd:string ;
    dct:description "Data is published by the data subject"@en ;
    rdfs:comment "This refers to where that data was made publicly available by the data subject. An example of this would be a social media profile that the data subject has made publicly accessible."@en ;
    rdfs:isDefinedBy dpvo: ;
    sw:term_status "accepted"@en .

dpvo:DataRedaction a owl:Class ;
    rdfs:label "Data Redaction"@en ;
    dct:created "2020-10-01"^^xsd:date ;
    dct:creator "Harshvardhan J. Pandit"^^xsd:string ;
    dct:description "Removal of sensitive information from a data or document"@en ;
    rdfs:isDefinedBy dpvo: ;
    rdfs:subClassOf dpvo:DataSanitisationTechnique ;
    sw:term_status "accepted"@en .

dpvo:DataSubProcessor a owl:Class ;
    rdfs:label "Data Sub-Processor"@en ;
    dct:created "2020-11-25"^^xsd:date ;
    dct:creator "Harshvardhan J. Pandit"^^xsd:string ;
    dct:description "A 'sub-processor' is a processor engaged by another processor"@en ;
    rdfs:comment "sub-processor' is a commonly used term similar to 'sub-contractor' and does not have a specific legal definition"@en ;
    rdfs:isDefinedBy dpvo: ;
    rdfs:subClassOf dpvo:DataProcessor ;
    sw:term_status "accepted"@en .

dpvo:DataSubjectRight a owl:Class ;
    rdfs:label "Data Subject Right"@en ;
    dct:created "2020-11-18"^^xsd:date ;
    dct:creator "Beatriz Esteves"^^xsd:string,
        "Georg P Krog"^^xsd:string,
        "Harshvardhan Pandit"^^xsd:string ;
    dct:description "The rights applicable or provided to a Data Subject"@en ;
    rdfs:comment "Based on use of definitions, the notion of 'Data Subject Right' can be equivalent to 'Individual Right' or 'Right of a Person'"@en ;
    rdfs:isDefinedBy dpvo: ;
    rdfs:subClassOf dpvo:Right ;
    sw:term_status "accepted"@en .

dpvo:DataTransferImpactAssessment a owl:Class ;
    rdfs:label "Data Transfer Impact Assessment"@en ;
    dct:created "2021-09-08"^^xsd:date ;
    dct:creator "Georg P Krog"^^xsd:string,
        "Harshvardhan J. Pandit"^^xsd:string,
        "Paul Ryan"^^xsd:string ;
    dct:description "Impact Assessment for conducting data transfers"@en ;
    rdfs:isDefinedBy dpvo: ;
    rdfs:subClassOf dpvo:ImpactAssessment ;
    sw:term_status "accepted"@en .

dpvo:DataTransferLegalBasis a owl:Class ;
    rdfs:label "Data Transfer Legal Basis"@en ;
    dct:created "2021-09-08"^^xsd:date ;
    dct:creator "David Hickey"^^xsd:string,
        "Georg P Krogg"^^xsd:string ;
    dct:description "Specific or special categories and instances of legal basis intended for justifying data transfers"@en ;
    rdfs:isDefinedBy dpvo: ;
    rdfs:subClassOf dpvo:LegalBasis ;
    sw:term_status "accepted"@en .

dpvo:DecentralisedLocations a owl:Class ;
    rdfs:label "Decentralised Locations"@en ;
    dct:created "2022-06-15"^^xsd:date ;
    dct:creator "Harshvardhan J. Pandit"^^xsd:string ;
    dct:description "Location that is spread across multiple separate areas with no distinction between their importance"@en ;
    dct:modified "2020-10-05"^^xsd:date ;
    rdfs:isDefinedBy dpvo: ;
    rdfs:subClassOf dpvo:LocationFixture ;
    sw:term_status "modified"@en .

dpvo:DeliveryOfGoods a owl:Class ;
    rdfs:label "Delivery of Goods"@en ;
    dct:created "2019-04-05"^^xsd:date ;
    dct:creator "Axel Polleres"^^xsd:string,
        "Elmar Kiesling"^^xsd:string,
        "Fajar Ekaputra"^^xsd:string,
        "Harshvardhan J. Pandit"^^xsd:string,
        "Javier Fernandez"^^xsd:string,
        "Simon Steyskal"^^xsd:string ;
    dct:description "Purposes associated with delivering goods and services requested or asked by consumer"@en ;
    rdfs:isDefinedBy dpvo: ;
    rdfs:seeAlso svpu:Delivery ;
    rdfs:subClassOf dpvo:RequestedServiceProvision ;
    sw:term_status "accepted"@en .

dpvo:DesignStandard a owl:Class ;
    rdfs:label "Design Standard"@en ;
    dct:created "2019-04-05"^^xsd:date ;
    dct:creator "Axel Polleres"^^xsd:string,
        "Harshvardhan J. Pandit"^^xsd:string,
        "Mark Lizar"^^xsd:string,
        "Rob Brennan"^^xsd:string ;
    dct:description "A set of rules or guidelines outlining criterias for design"@en ;
    rdfs:isDefinedBy dpvo: ;
    rdfs:subClassOf dpvo:GuidelinesPrinciple ;
    sw:term_status "accepted"@en .

dpvo:Destruct a owl:Class ;
    rdfs:label "Destruct"@en ;
    dct:created "2019-05-07"^^xsd:date ;
    dct:description "to process data in a way it no longer exists or cannot be repaired"@en ;
    dct:source <https://eur-lex.europa.eu/eli/reg/2016/679/art_4/par_2/oj> ;
    rdfs:isDefinedBy dpvo: ;
    rdfs:subClassOf dpvo:Remove ;
    sw:term_status "accepted"@en .

dpvo:DeterministicPseudonymisation a owl:Class ;
    rdfs:label "Deterministic Pseudonymisation"@en ;
    dct:created "2022-08-17"^^xsd:date ;
    dct:creator "Harshvardhan J. Pandit"^^xsd:string ;
    dct:description "Pseudonymisation achieved through a deterministic function"@en ;
    dct:source <https://www.enisa.europa.eu/publications/data-pseudonymisation-advanced-techniques-and-use-cases> ;
    rdfs:isDefinedBy dpvo: ;
    rdfs:subClassOf dpvo:Pseudonymisation ;
    sw:term_status "accepted"@en .

dpvo:Detriment a owl:Class ;
    rdfs:label "Detriment"@en ;
    dct:created "2022-03-23"^^xsd:date ;
    dct:creator "Beatriz Esteves"^^xsd:string,
        "Fajar Ekaputra"^^xsd:string,
        "Georg P Krog"^^xsd:string,
        "Harshvardhan J. Pandit"^^xsd:string,
        "Julian Flake"^^xsd:string ;
    dct:description "Impact that acts as or causes detriments"@en ;
    rdfs:isDefinedBy dpvo: ;
    rdfs:subClassOf dpvo:Impact ;
    sw:term_status "accepted"@en .

dpvo:DifferentialPrivacy a owl:Class ;
    rdfs:label "Differential Privacy"@en ;
    dct:created "2022-08-17"^^xsd:date ;
    dct:creator "Harshvardhan J. Pandit"^^xsd:string ;
    dct:description "Utilisation of differential privacy where information is shared as patterns or groups to withold individual elements"@en ;
    dct:source <https://www.enisa.europa.eu/publications/data-protection-engineering> ;
    rdfs:isDefinedBy dpvo: ;
    rdfs:subClassOf dpvo:CryptographicMethods ;
    sw:term_status "accepted"@en .

dpvo:DigitalRightsManagement a owl:Class ;
    rdfs:label "Digital Rights Management"@en ;
    dct:created "2022-08-17"^^xsd:date ;
    dct:creator "Harshvardhan J. Pandit"^^xsd:string ;
    dct:description "Management of access, use, and other operations associated with digital content"@en ;
    dct:source <https://www.enisa.europa.eu/publications/reference-incident-classification-taxonomy/> ;
    rdfs:isDefinedBy dpvo: ;
    rdfs:subClassOf dpvo:TechnicalMeasure ;
    sw:term_status "accepted"@en .

dpvo:DigitalSignatures a owl:Class ;
    rdfs:label "Digital Signatures"@en ;
    dct:created "2022-08-17"^^xsd:date ;
    dct:creator "Harshvardhan J. Pandit"^^xsd:string ;
    dct:description "Expression and authentication of identity through digital information containing cryptographic signatures"@en ;
    dct:source <https://www.enisa.europa.eu/publications/reference-incident-classification-taxonomy/> ;
    rdfs:isDefinedBy dpvo: ;
    rdfs:subClassOf dpvo:CryptographicMethods ;
    sw:term_status "accepted"@en .

dpvo:DirectMarketing a owl:Class ;
    rdfs:label "Direct Marketing"@en ;
    dct:created "2020-11-04"^^xsd:date ;
    dct:creator "Beatriz Esteves"^^xsd:string,
        "Georg P Krog"^^xsd:string,
        "Harshvardhan J. Pandit"^^xsd:string ;
    dct:description "Purposes associated with conducting direct marketing i.e. marketing communicated directly to the individual"@en ;
    rdfs:isDefinedBy dpvo: ;
    rdfs:subClassOf dpvo:Marketing ;
    sw:term_status "accepted"@en .

dpvo:DisasterRecoveryProcedures a owl:Class ;
    rdfs:label "Disaster Recovery Procedures"@en ;
    dct:created "2022-08-17"^^xsd:date ;
    dct:creator "Harshvardhan J. Pandit"^^xsd:string ;
    dct:description "Procedures related to management of disasters and recovery"@en ;
    dct:source <https://www.enisa.europa.eu/publications/5g-cybersecurity-standards> ;
    rdfs:isDefinedBy dpvo: ;
    rdfs:subClassOf dpvo:GovernanceProcedures ;
    sw:term_status "accepted"@en .

dpvo:DiscloseByTransmission a owl:Class ;
    rdfs:label "Disclose by Transmission"@en ;
    dct:created "2019-05-07"^^xsd:date ;
    dct:description "to disclose data by means of transmission"@en ;
    dct:source <https://eur-lex.europa.eu/eli/reg/2016/679/art_4/par_2/oj> ;
    rdfs:isDefinedBy dpvo: ;
    rdfs:subClassOf dpvo:Disclose ;
    sw:term_status "accepted"@en .

dpvo:DisputeManagement a owl:Class ;
    rdfs:label "Dispute Management"@en ;
    dct:created "2021-09-08"^^xsd:date ;
    dct:creator "Beatriz Esteves"^^xsd:string,
        "Georg P Krog"^^xsd:string,
        "Harshvardhan J. Pandit"^^xsd:string ;
    dct:description "Purposes associated with activities that manage disputes by natural persons, private bodies, or public authorities relevant to organisation"@en ;
    dct:source <https://www.privacycommission.be/nl/model-voor-een-register-van-de-verwerkingsactiviteiten> ;
    rdfs:isDefinedBy dpvo: ;
    rdfs:subClassOf dpvo:OrganisationGovernance ;
    sw:term_status "accepted"@en .

dpvo:Disseminate a owl:Class ;
    rdfs:label "Disseminate"@en ;
    dct:created "2019-05-07"^^xsd:date ;
    dct:description "to spread data throughout"@en ;
    dct:source <https://eur-lex.europa.eu/eli/reg/2016/679/art_4/par_2/oj> ;
    rdfs:isDefinedBy dpvo: ;
    rdfs:subClassOf dpvo:Disclose ;
    sw:term_status "accepted"@en .

dpvo:DistributedSystemSecurity a owl:Class ;
    rdfs:label "Distributed System Security"@en ;
    dct:created "2022-08-17"^^xsd:date ;
    dct:creator "Harshvardhan J. Pandit"^^xsd:string ;
    dct:description "Security implementations provided using or over a distributed system"@en ;
    dct:source <https://www.enisa.europa.eu/publications/reference-incident-classification-taxonomy/> ;
    rdfs:isDefinedBy dpvo: ;
    rdfs:subClassOf dpvo:SecurityMethod ;
    sw:term_status "accepted"@en .

dpvo:DocumentRandomisedPseudonymisation a owl:Class ;
    rdfs:label "Document Randomised Pseudonymisation"@en ;
    dct:created "2022-08-17"^^xsd:date ;
    dct:creator "Harshvardhan J. Pandit"^^xsd:string ;
    dct:description "Use of randomised pseudonymisation where the same elements are assigned different values in the same document or database"@en ;
    dct:source <https://www.enisa.europa.eu/publications/data-pseudonymisation-advanced-techniques-and-use-cases> ;
    rdfs:isDefinedBy dpvo: ;
    rdfs:subClassOf dpvo:Pseudonymisation ;
    sw:term_status "accepted"@en .

dpvo:DocumentSecurity a owl:Class ;
    rdfs:label "Document Security"@en ;
    dct:created "2022-08-17"^^xsd:date ;
    dct:creator "Harshvardhan J. Pandit"^^xsd:string ;
    dct:description "Security measures enacted over documents to protect against tampering or restrict access"@en ;
    dct:source <https://www.enisa.europa.eu/publications/reference-incident-classification-taxonomy/> ;
    rdfs:isDefinedBy dpvo: ;
    rdfs:subClassOf dpvo:SecurityMethod ;
    sw:term_status "accepted"@en .

dpvo:EconomicUnion a owl:Class ;
    rdfs:label "Economic Union"@en ;
    dct:created "2022-01-19"^^xsd:date ;
    dct:creator "Harshvardhan J. Pandit"^^xsd:string ;
    dct:description "A political union of two or more countries based on economic or trade agreements"@en ;
    rdfs:isDefinedBy dpvo: ;
    rdfs:subClassOf dpvo:Location ;
    sw:term_status "accepted"@en .

dpvo:EducationalTraining a owl:Class ;
    rdfs:label "Educational Training"@en ;
    dct:created "2022-08-17"^^xsd:date ;
    dct:creator "Harshvardhan J. Pandit"^^xsd:string ;
    dct:description "Training methods that are intended to provide education on topic(s)"@en ;
    dct:source <https://www.enisa.europa.eu/publications/reference-incident-classification-taxonomy/> ;
    rdfs:isDefinedBy dpvo: ;
    rdfs:subClassOf dpvo:StaffTraining ;
    sw:term_status "accepted"@en .

dpvo:EffectivenessDeterminationProcedures a owl:Class ;
    rdfs:label "Effectiveness Determination Procedures"@en ;
    dct:created "2022-08-17"^^xsd:date ;
    dct:creator "Harshvardhan J. Pandit"^^xsd:string ;
    dct:description "Procedures intended to determine effectiveness of other measures"@en ;
    dct:source <https://www.enisa.europa.eu/publications/5g-cybersecurity-standards> ;
    rdfs:isDefinedBy dpvo: ;
    rdfs:subClassOf dpvo:Assessment ;
    sw:term_status "accepted"@en .

dpvo:ElderlyDataSubject a owl:Class ;
    rdfs:label "Elderly Data Subject"@en ;
    dct:created "2022-06-15"^^xsd:date ;
    dct:creator "Georg P Krog"^^xsd:string ;
    dct:description "Data subjects that are considered elderly (i.e. based on age)"@en ;
    rdfs:isDefinedBy dpvo: ;
    rdfs:subClassOf dpvo:VulnerableDataSubject ;
    sw:term_status "accepted"@en .

dpvo:Employee a owl:Class ;
    rdfs:label "Employee"@en ;
    dct:created "2022-04-06"^^xsd:date ;
    dct:creator "Beatriz Esteves"^^xsd:string,
        "Georg P. Krog"^^xsd:string,
        "Harshvardhan J. Pandit"^^xsd:string,
        "Julian Flake"^^xsd:string,
        "Paul Ryan"^^xsd:string ;
    dct:description "Data subjects that are employees"@en ;
    rdfs:isDefinedBy dpvo: ;
    rdfs:subClassOf dpvo:DataSubject ;
    sw:term_status "accepted"@en .

dpvo:EncryptionAtRest a owl:Class ;
    rdfs:label "Encryption at Rest"@en ;
    dct:created "2019-04-05"^^xsd:date ;
    dct:creator "Axel Polleres"^^xsd:string,
        "Harshvardhan J. Pandit"^^xsd:string,
        "Mark Lizar"^^xsd:string,
        "Rob Brennan"^^xsd:string ;
    dct:description "Encryption of data when being stored (persistent encryption)"@en ;
    rdfs:isDefinedBy dpvo: ;
    rdfs:subClassOf dpvo:Encryption ;
    sw:term_status "accepted"@en .

dpvo:EncryptionInTransfer a owl:Class ;
    rdfs:label "Encryption in Transfer"@en ;
    dct:created "2019-04-05"^^xsd:date ;
    dct:creator "Axel Polleres"^^xsd:string,
        "Harshvardhan J. Pandit"^^xsd:string,
        "Mark Lizar"^^xsd:string,
        "Rob Brennan"^^xsd:string ;
    dct:description "Encryption of data in transit e.g. when being transferred from one location to another, including sharing"@en ;
    rdfs:isDefinedBy dpvo: ;
    rdfs:subClassOf dpvo:Encryption ;
    sw:term_status "accepted"@en .

dpvo:EncryptionInUse a owl:Class ;
    rdfs:label "Encryption in Use"@en ;
    dct:created "2022-10-22"^^xsd:date ;
    dct:creator "Harshvardhan J. Pandit"^^xsd:string ;
    dct:description "Encryption of data when it is being used"@en ;
    rdfs:isDefinedBy dpvo: ;
    rdfs:subClassOf dpvo:Encryption ;
    sw:term_status "accepted"@en .

dpvo:EndToEndEncryption a owl:Class ;
    rdfs:label "End-to-End Encryption (E2EE)"@en ;
    dct:created "2022-08-17"^^xsd:date ;
    dct:creator "Harshvardhan J. Pandit"^^xsd:string ;
    dct:description "Encrypted communications where data is encrypted by the sender and decrypted by the intended receiver to prevent access to any third party"@en ;
    dct:source <https://www.enisa.europa.eu/publications/data-protection-engineering> ;
    rdfs:isDefinedBy dpvo: ;
    rdfs:subClassOf dpvo:Encryption ;
    sw:term_status "accepted"@en .

dpvo:EndlessDuration a owl:NamedIndividual,
        dpvo:Duration ;
    rdfs:label "Endless Duration"@en ;
    dct:created "2022-06-15"^^xsd:date ;
    dct:creator "Harshvardhan J. Pandit"^^xsd:string ;
    dct:description "Duration that is (known or intended to be) open ended or without an end"@en ;
    dct:modified "2020-10-05"^^xsd:date ;
    rdfs:isDefinedBy dpvo: ;
    sw:term_status "modified"@en .

dpvo:EnforceAccessControl a owl:Class ;
    rdfs:label "Enforce Access Control"@en ;
    dct:created "2019-04-05"^^xsd:date ;
    dct:creator "Axel Polleres"^^xsd:string,
        "Elmar Kiesling"^^xsd:string,
        "Fajar Ekaputra"^^xsd:string,
        "Harshvardhan J. Pandit"^^xsd:string,
        "Javier Fernandez"^^xsd:string,
        "Simon Steyskal"^^xsd:string ;
    dct:description "Purposes associated with conducting or enforcing access control as a form of security"@en ;
    rdfs:comment "Was previously \"Access Control\". Prefixed to distinguish from Technical Measure."@en ;
    rdfs:isDefinedBy dpvo: ;
    rdfs:seeAlso svpu:Login ;
    rdfs:subClassOf dpvo:EnforceSecurity ;
    sw:term_status "accepted"@en .

dpvo:EnterIntoContract a owl:Class ;
    rdfs:label "Enter Into Contract"@en ;
    dct:created "2021-04-07"^^xsd:date ;
    dct:creator "Georg P Krog"^^xsd:string,
        "Harshvardhan J. Pandit"^^xsd:string,
        "Paul Ryan"^^xsd:string ;
    dct:description "Processing necessary to enter into contract"@en ;
    rdfs:isDefinedBy dpvo: ;
    rdfs:subClassOf dpvo:Contract ;
    sw:term_status "accepted"@en .

dpvo:Erase a owl:Class ;
    rdfs:label "Erase"@en ;
    dct:created "2019-05-07"^^xsd:date ;
    dct:description "to delete data"@en ;
    dct:source <https://eur-lex.europa.eu/eli/reg/2016/679/art_4/par_2/oj> ;
    rdfs:isDefinedBy dpvo: ;
    rdfs:subClassOf dpvo:Remove ;
    sw:term_status "accepted"@en .

dpvo:EstablishContractualAgreement a owl:Class ;
    rdfs:label "Establish Contractual Agreement"@en ;
    dct:created "2022-11-09"^^xsd:date ;
    dct:creator "Georg P Krog"^^xsd:string,
        "Harshvardhan J. Pandit"^^xsd:string ;
    dct:description "Purposes associated with carrying out data processing to establish an agreement, such as for entering into a contract"@en ;
    rdfs:isDefinedBy dpvo: ;
    rdfs:subClassOf dpvo:Purpose ;
    sw:term_status "accepted"@en .

dpvo:EvaluationOfIndividuals a owl:Class ;
    rdfs:label "Evaluation of Individuals"@en ;
    dct:created "2022-10-22"^^xsd:date ;
    dct:creator "Harshvardhan J. Pandit"^^xsd:string ;
    dct:description "Processing that involves evaluation of individuals"@en ;
    dct:modified "2022-11-30"^^xsd:date ;
    dct:source <https://eur-lex.europa.eu/eli/reg/2016/679/art_4/par_2/oj> ;
    rdfs:isDefinedBy dpvo: ;
    rdfs:subClassOf dpvo:EvaluationScoring ;
    sw:term_status "modified"@en .

dpvo:ExplicitlyExpressedConsent a owl:Class ;
    rdfs:label "Explicitly Expressed Consent"@en ;
    dct:created "2022-06-21"^^xsd:date ;
    dct:creator "Georg P Krog"^^xsd:string,
        "Harshvardhan J. Pandit"^^xsd:string,
        "Julian Flake"^^xsd:string,
        "Paul Ryan"^^xsd:string ;
    dct:description "Consent that is expressed through an explicit action solely conveying a consenting decision"@en ;
    rdfs:comment "Explicitly expressed consent is a more specific form of Expressed consent where the action taken must 'explicitly' relate to only the consent decision. Expressed consent where the consenting is part of other matters therefore cannot satisfy the requirements of explicitly expressed consent. An example of explicit action expressing the consenting decision is a button on a web form where the form only relates to consent, or it is accompanied with suitable text that reiterates what the consenting decision is about"@en ;
    rdfs:isDefinedBy dpvo: ;
    rdfs:subClassOf dpvo:ExpressedConsent ;
    sw:term_status "accepted"@en .

dpvo:FederatedLocations a owl:Class ;
    rdfs:label "Federated Locations"@en ;
    dct:created "2022-06-15"^^xsd:date ;
    dct:creator "Harshvardhan J. Pandit"^^xsd:string ;
    dct:description "Location that is federated across multiple separate areas with designation of a primary or central location"@en ;
    dct:modified "2020-10-05"^^xsd:date ;
    rdfs:isDefinedBy dpvo: ;
    rdfs:subClassOf dpvo:LocationFixture ;
    sw:term_status "modified"@en .

dpvo:FileSystemSecurity a owl:Class ;
    rdfs:label "File System Security"@en ;
    dct:created "2022-08-17"^^xsd:date ;
    dct:creator "Harshvardhan J. Pandit"^^xsd:string ;
    dct:description "Security implemented over a file system"@en ;
    dct:source <https://www.enisa.europa.eu/publications/reference-incident-classification-taxonomy/> ;
    rdfs:isDefinedBy dpvo: ;
    rdfs:subClassOf dpvo:SecurityMethod ;
    sw:term_status "accepted"@en .

dpvo:Filter a owl:Class ;
    rdfs:label "Filter"@en ;
    dct:created "2022-06-15"^^xsd:date ;
    dct:creator "Georg P Krog"^^xsd:string,
        "Harshvardhan J. Pandit"^^xsd:string ;
    dct:description "to filter or keep data for some criteria"@en ;
    rdfs:isDefinedBy dpvo: ;
    rdfs:subClassOf dpvo:Transform ;
    sw:term_status "accepted"@en .

dpvo:FixedMultipleLocations a owl:Class ;
    rdfs:label "Fixed Multiple Locations"@en ;
    dct:created "2022-06-15"^^xsd:date ;
    dct:creator "Harshvardhan J. Pandit"^^xsd:string ;
    dct:description "Location that is fixed with multiple places e.g. multiple cities"@en ;
    dct:modified "2020-10-05"^^xsd:date ;
    rdfs:isDefinedBy dpvo: ;
    rdfs:subClassOf dpvo:FixedLocation ;
    sw:term_status "modified"@en .

dpvo:FixedOccurencesDuration a owl:Class ;
    rdfs:label "Fixed Occurences Duration"@en ;
    dct:created "2022-06-15"^^xsd:date ;
    dct:creator "Harshvardhan J. Pandit"^^xsd:string ;
    dct:description "Duration that takes place a fixed number of times e.g. 3 times"@en ;
    dct:modified "2020-10-05"^^xsd:date ;
    rdfs:isDefinedBy dpvo: ;
    rdfs:subClassOf dpvo:Duration ;
    sw:term_status "modified"@en .

dpvo:FixedSingularLocation a owl:Class ;
    rdfs:label "Fixed Singular Location"@en ;
    dct:created "2022-06-15"^^xsd:date ;
    dct:creator "Harshvardhan J. Pandit"^^xsd:string ;
    dct:description "Location that is fixed at a specific place e.g. a city"@en ;
    dct:modified "2020-10-05"^^xsd:date ;
    rdfs:isDefinedBy dpvo: ;
    rdfs:subClassOf dpvo:FixedLocation ;
    sw:term_status "modified"@en .

dpvo:ForProfitOrganisation a owl:Class ;
    rdfs:label "For-Profit Organisation"@en ;
    dct:created "2022-02-02"^^xsd:date ;
    dct:creator "Harshvardhan J. Pandit"^^xsd:string ;
    dct:description "An organisation that aims to achieve profit as its primary goal"@en ;
    dct:modified "2020-10-05"^^xsd:date ;
    rdfs:isDefinedBy dpvo: ;
    rdfs:subClassOf dpvo:Organisation ;
    sw:term_status "modified"@en .

dpvo:FulfilmentOfContractualObligation a owl:Class ;
    rdfs:label "Fulfilment of Contractual Obligation"@en ;
    dct:created "2022-11-09"^^xsd:date ;
    dct:creator "Georg P Krog"^^xsd:string,
        "Harshvardhan J. Pandit"^^xsd:string ;
    dct:description "Purposes associated with carrying out data processing to fulfill a contractual obligation"@en ;
    rdfs:isDefinedBy dpvo: ;
    rdfs:subClassOf dpvo:FulfilmentOfObligation ;
    sw:term_status "accepted"@en .

dpvo:FullyAutomatedProcessing a owl:NamedIndividual,
        dpvo:AutomationOfProcessing ;
    rdfs:label "Fully Automated Processing"@en ;
    dct:created "2022-06-15"^^xsd:date ;
    dct:creator "Harshvardhan J. Pandit"^^xsd:string ;
    dct:description "Processing that is fully automated"@en ;
    rdfs:isDefinedBy dpvo: ;
    sw:term_status "accepted"@en .

dpvo:FullyRandomisedPseudonymisation a owl:Class ;
    rdfs:label "Fully Randomised Pseudonymisation"@en ;
    dct:created "2022-08-17"^^xsd:date ;
    dct:creator "Harshvardhan J. Pandit"^^xsd:string ;
    dct:description "Use of randomised pseudonymisation where the same elements are assigned different values each time they occur"@en ;
    dct:source <https://www.enisa.europa.eu/publications/data-pseudonymisation-advanced-techniques-and-use-cases> ;
    rdfs:isDefinedBy dpvo: ;
    rdfs:subClassOf dpvo:Pseudonymisation ;
    sw:term_status "accepted"@en .

dpvo:Generate a owl:Class ;
    rdfs:label "Generate"@en ;
    dct:created "2022-04-20"^^xsd:date ;
    dct:creator "Harshvardhan J. Pandit"^^xsd:string ;
    dct:description "to generate or create data"@en ;
    rdfs:isDefinedBy dpvo: ;
    rdfs:subClassOf dpvo:Obtain ;
    sw:term_status "accepted"@en .

dpvo:GlobalScale a owl:NamedIndividual,
        dpvo:GeographicCoverage ;
    rdfs:label "Global Scale"@en ;
    dct:created "2022-06-15"^^xsd:date ;
    dct:creator "Harshvardhan J. Pandit"^^xsd:string ;
    dct:description "Geographic coverage spanning the entire globe"@en ;
    rdfs:isDefinedBy dpvo: ;
    sw:term_status "accepted"@en .

dpvo:GuardianOfDataSubject a owl:Class ;
    rdfs:label "Guardian(s) of Data Subject"@en ;
    dct:created "2022-08-03"^^xsd:date ;
    dct:creator "Georg P Krog"^^xsd:string ;
    dct:description "Guardian(s) of data subjects such as children"@en ;
    rdfs:isDefinedBy dpvo: ;
    rdfs:subClassOf dpvo:DataSubject ;
    sw:term_status "accepted"@en .

dpvo:HardwareSecurityProtocols a owl:Class ;
    rdfs:label "Hardware Security Protocols"@en ;
    dct:created "2022-08-17"^^xsd:date ;
    dct:creator "Harshvardhan J. Pandit"^^xsd:string ;
    dct:description "Security protocols implemented at or within hardware"@en ;
    dct:source <https://www.enisa.europa.eu/publications/reference-incident-classification-taxonomy/> ;
    rdfs:isDefinedBy dpvo: ;
    rdfs:subClassOf dpvo:SecurityMethod ;
    sw:term_status "accepted"@en .

dpvo:Harm a owl:Class ;
    rdfs:label "Harm"@en ;
    dct:created "2022-08-13"^^xsd:date ;
    dct:creator "Beatriz Esteves"^^xsd:string,
        "Fajar Ekaputra"^^xsd:string,
        "Georg P Krog"^^xsd:string,
        "Harshvardhan J. Pandit"^^xsd:string,
        "Julian Flake"^^xsd:string ;
    dct:description "Impact that acts as or causes harms"@en ;
    rdfs:isDefinedBy dpvo: ;
    rdfs:subClassOf dpvo:Damage ;
    sw:term_status "changed"@en .

dpvo:HashFunctions a owl:Class ;
    rdfs:label "Hash Functions"@en ;
    dct:created "2022-08-17"^^xsd:date ;
    dct:creator "Harshvardhan J. Pandit"^^xsd:string ;
    dct:description "Use of hash functions to map information or to retrieve a prior categorisation"@en ;
    dct:source <https://www.enisa.europa.eu/publications/reference-incident-classification-taxonomy/> ;
    rdfs:isDefinedBy dpvo: ;
    rdfs:subClassOf dpvo:CryptographicMethods ;
    sw:term_status "accepted"@en .

dpvo:HashMessageAuthenticationCode a owl:Class ;
    rdfs:label "Hash-based Message Authentication Code (HMAC)"@en ;
    dct:created "2022-08-17"^^xsd:date ;
    dct:creator "Harshvardhan J. Pandit"^^xsd:string ;
    dct:description "Use of HMAC where message authentication code (MAC) utilise a cryptographic hash function and a secret cryptographic key"@en ;
    dct:source <https://www.enisa.europa.eu/publications/5g-cybersecurity-standards> ;
    rdfs:isDefinedBy dpvo: ;
    rdfs:subClassOf dpvo:CryptographicAuthentication ;
    sw:term_status "accepted"@en .

dpvo:HomomorphicEncryption a owl:Class ;
    rdfs:label "Homomorphic Encryption"@en ;
    dct:created "2022-08-17"^^xsd:date ;
    dct:creator "Harshvardhan J. Pandit"^^xsd:string ;
    dct:description "Use of Homomorphic encryption that permits computations on encrypted data without decrypting it"@en ;
    dct:source <https://www.enisa.europa.eu/publications/reference-incident-classification-taxonomy/> ;
    rdfs:isDefinedBy dpvo: ;
    rdfs:subClassOf dpvo:CryptographicMethods ;
    sw:term_status "accepted"@en .

dpvo:HugeDataVolume a owl:NamedIndividual,
        dpvo:DataVolume ;
    rdfs:label "Huge Data Volume"@en ;
    dct:created "2022-06-15"^^xsd:date ;
    dct:creator "Harshvardhan J. Pandit"^^xsd:string ;
    dct:description "Data volume that is considered huge or more than large within the context"@en ;
    rdfs:isDefinedBy dpvo: ;
    sw:term_status "accepted"@en .

dpvo:HugeScaleOfDataSubjects a owl:NamedIndividual,
        dpvo:DataSubjectScale ;
    rdfs:label "Huge Scale Of Data Subjects"@en ;
    dct:created "2022-06-15"^^xsd:date ;
    dct:creator "Harshvardhan J. Pandit"^^xsd:string ;
    dct:description "Scale of data subjects considered huge or more than large within the context"@en ;
    rdfs:isDefinedBy dpvo: ;
    sw:term_status "accepted"@en .

dpvo:IdentityManagementMethod a owl:Class ;
    rdfs:label "Identity Management Method"@en ;
    dct:created "2022-08-17"^^xsd:date ;
    dct:creator "Harshvardhan J. Pandit"^^xsd:string ;
    dct:description "Management of identity and identity-based processes"@en ;
    dct:source <https://www.enisa.europa.eu/publications/reference-incident-classification-taxonomy/> ;
    rdfs:isDefinedBy dpvo: ;
    rdfs:subClassOf dpvo:AuthorisationProcedure ;
    sw:term_status "accepted"@en .

dpvo:IdentityVerification a owl:Class ;
    rdfs:label "Identity Verification"@en ;
    dct:created "2019-04-05"^^xsd:date ;
    dct:creator "Axel Polleres"^^xsd:string,
        "Elmar Kiesling"^^xsd:string,
        "Fajar Ekaputra"^^xsd:string,
        "Harshvardhan J. Pandit"^^xsd:string,
        "Javier Fernandez"^^xsd:string,
        "Simon Steyskal"^^xsd:string ;
    dct:description "Purposes associated with verifying or authorising identity as a form of security"@en ;
    rdfs:isDefinedBy dpvo: ;
    rdfs:subClassOf dpvo:EnforceSecurity ;
    sw:term_status "accepted"@en .

dpvo:Immigrant a owl:Class ;
    rdfs:label "Immigrant"@en ;
    dct:created "2022-04-06"^^xsd:date ;
    dct:creator "Beatriz Esteves"^^xsd:string,
        "Georg P. Krog"^^xsd:string,
        "Harshvardhan J. Pandit"^^xsd:string,
        "Julian Flake"^^xsd:string,
        "Paul Ryan"^^xsd:string ;
    dct:description "Data subjects that are immigrants (for a jurisdiction)"@en ;
    rdfs:isDefinedBy dpvo: ;
    rdfs:subClassOf dpvo:DataSubject ;
    sw:term_status "accepted"@en .

dpvo:ImpliedConsent a owl:Class ;
    rdfs:label "Implied Consent"@en ;
    dct:created "2022-06-21"^^xsd:date ;
    dct:creator "Georg P Krog"^^xsd:string,
        "Harshvardhan J. Pandit"^^xsd:string,
        "Julian Flake"^^xsd:string,
        "Paul Ryan"^^xsd:string ;
    dct:description "Consent that is implied indirectly through an action not associated solely with conveying a consenting decision"@en ;
    rdfs:comment "Implied consent is expected to also be Informed Consent. An example is a CCTV notice outside a monitored area that informs the individuals that by walking in they would be consenting to the use of camera for surveillance."@en ;
    rdfs:isDefinedBy dpvo: ;
    rdfs:subClassOf dpvo:InformedConsent ;
    sw:term_status "accepted"@en .

dpvo:ImproveExistingProductsAndServices a owl:Class ;
    rdfs:label "Improve Existing Products and Services"@en ;
    dct:created "2019-04-05"^^xsd:date ;
    dct:creator "Axel Polleres"^^xsd:string,
        "Elmar Kiesling"^^xsd:string,
        "Fajar Ekaputra"^^xsd:string,
        "Harshvardhan J. Pandit"^^xsd:string,
        "Javier Fernandez"^^xsd:string,
        "Simon Steyskal"^^xsd:string ;
    dct:description "Purposes associated with improving existing products and services"@en ;
    rdfs:isDefinedBy dpvo: ;
    rdfs:subClassOf dpvo:OptimisationForController ;
    sw:term_status "accepted"@en .

dpvo:ImproveInternalCRMProcesses a owl:Class ;
    rdfs:label "Improve Internal CRM Processes"@en ;
    dct:created "2019-04-05"^^xsd:date ;
    dct:creator "Axel Polleres"^^xsd:string,
        "Elmar Kiesling"^^xsd:string,
        "Fajar Ekaputra"^^xsd:string,
        "Harshvardhan J. Pandit"^^xsd:string,
        "Javier Fernandez"^^xsd:string,
        "Simon Steyskal"^^xsd:string ;
    dct:description "Purposes associated with improving customer-relationship management (CRM) processes"@en ;
    rdfs:isDefinedBy dpvo: ;
    rdfs:subClassOf dpvo:CustomerRelationshipManagement,
        dpvo:OptimisationForController ;
    sw:term_status "accepted"@en .

dpvo:IncidentManagementProcedures a owl:Class ;
    rdfs:label "Incident Management Procedures"@en ;
    dct:created "2022-08-17"^^xsd:date ;
    dct:creator "Harshvardhan J. Pandit"^^xsd:string ;
    dct:description "Procedures related to management of incidents"@en ;
    dct:source <https://www.enisa.europa.eu/publications/5g-cybersecurity-standards> ;
    rdfs:isDefinedBy dpvo: ;
    rdfs:subClassOf dpvo:GovernanceProcedures ;
    sw:term_status "accepted"@en .

dpvo:IncidentReportingCommunication a owl:Class ;
    rdfs:label "Incident Reporting Communication"@en ;
    dct:created "2022-08-17"^^xsd:date ;
    dct:creator "Harshvardhan J. Pandit"^^xsd:string ;
    dct:description "Procedures related to management of incident reporting"@en ;
    dct:source <https://www.enisa.europa.eu/publications/5g-cybersecurity-standards> ;
    rdfs:isDefinedBy dpvo: ;
    rdfs:subClassOf dpvo:GovernanceProcedures ;
    sw:term_status "accepted"@en .

dpvo:IncorrectData a owl:Class ;
    rdfs:label "Incorrect Data"@en ;
    dct:created "2022-11-02"^^xsd:date ;
    dct:creator "Harshvardhan J. Pandit"^^xsd:string ;
    dct:description "Data that is known to be incorrect or inconsistent with some quality requirements"@en ;
    rdfs:isDefinedBy dpvo: ;
    rdfs:subClassOf dpvo:Data ;
    sw:term_status "accepted"@en .

dpvo:IncreaseServiceRobustness a owl:Class ;
    rdfs:label "Increase Service Robustness"@en ;
    dct:created "2019-04-05"^^xsd:date ;
    dct:creator "Axel Polleres"^^xsd:string,
        "Elmar Kiesling"^^xsd:string,
        "Fajar Ekaputra"^^xsd:string,
        "Harshvardhan J. Pandit"^^xsd:string,
        "Javier Fernandez"^^xsd:string,
        "Simon Steyskal"^^xsd:string ;
    dct:description "Purposes associated with improving robustness and resilience of services"@en ;
    rdfs:isDefinedBy dpvo: ;
    rdfs:subClassOf dpvo:OptimisationForController ;
    sw:term_status "accepted"@en .

dpvo:IndeterminateDuration a owl:NamedIndividual,
        dpvo:Duration ;
    rdfs:label "Indeterminate Duration"@en ;
    dct:created "2022-11-30"^^xsd:date ;
    dct:creator "Harshvardhan J. Pandit"^^xsd:string ;
    dct:description "Duration that is indeterminate or cannot be determined"@en ;
    rdfs:comment "Indeterminate means (exact or otherwise) information about the duration cannot be determined, which is distinct from 'EndlessDuration' where it is known (or decided) that the duration is open-ended or without an end."@en ;
    rdfs:isDefinedBy dpvo: ;
    sw:term_status "accepted"@en .

dpvo:IndustryConsortium a owl:Class ;
    rdfs:label "Industry Consortium"@en ;
    dct:created "2022-02-02"^^xsd:date ;
    dct:creator "Harshvardhan J. Pandit"^^xsd:string ;
    dct:description "A consortium established and comprising on industry organisations"@en ;
    dct:modified "2020-10-05"^^xsd:date ;
    dct:source <http://purl.org/adms> ;
    rdfs:isDefinedBy dpvo: ;
    rdfs:subClassOf dpvo:Organisation ;
    sw:term_status "modified"@en .

dpvo:Infer a owl:Class ;
    rdfs:label "Infer"@en ;
    dct:created "2022-04-20"^^xsd:date ;
    dct:creator "Harshvardhan J. Pandit"^^xsd:string ;
    dct:description "to infer data from existing data"@en ;
    dct:modified "2022-10-14"^^xsd:date ;
    rdfs:comment "Infer indicates data that is derived without it being present or obtainable from existing data. For data that is presented, and is 'extracted' or 'obtained' from existing data, see Derive."@en ;
    rdfs:isDefinedBy dpvo: ;
    rdfs:subClassOf dpvo:Derive ;
    sw:term_status "modified"@en .

dpvo:InferredPersonalData a owl:Class ;
    rdfs:label "Inferred Personal Data"@en ;
    dct:created "2022-01-19"^^xsd:date ;
    dct:creator "Harshvardhan J. Pandit"^^xsd:string ;
    dct:description "Personal Data that is obtained through inference from other data"@en ;
    rdfs:comment "Inferred Data is derived data generated from existing data, but which did not originally exist within it, e.g. inferring demographics from browsing history."@en ;
    rdfs:isDefinedBy dpvo: ;
    rdfs:subClassOf dpvo:DerivedPersonalData,
        dpvo:GeneratedPersonalData ;
    sw:term_status "accepted"@en .

dpvo:InformationFlowControl a owl:Class ;
    rdfs:label "Information Flow Control"@en ;
    dct:created "2022-08-17"^^xsd:date ;
    dct:creator "Harshvardhan J. Pandit"^^xsd:string ;
    dct:description "Use of measures to control information flows"@en ;
    dct:source <https://www.enisa.europa.eu/publications/reference-incident-classification-taxonomy/> ;
    rdfs:isDefinedBy dpvo: ;
    rdfs:subClassOf dpvo:TechnicalMeasure ;
    sw:term_status "accepted"@en .

dpvo:InformationSecurityPolicy a owl:Class ;
    rdfs:label "Information Security Policy"@en ;
    dct:created "2022-08-17"^^xsd:date ;
    dct:creator "Harshvardhan J. Pandit"^^xsd:string ;
    dct:description "Policy regarding security of information"@en ;
    dct:source <https://www.enisa.europa.eu/publications/5g-cybersecurity-standards> ;
    rdfs:isDefinedBy dpvo: ;
    rdfs:subClassOf dpvo:Policy ;
    sw:term_status "accepted"@en .

dpvo:InnovativeUseOfNewTechnologies a owl:Class ;
    rdfs:label "Innovative Use of New Technologies"@en ;
    dct:created "2020-11-04"^^xsd:date ;
    dct:creator "Harshvardhan J. Pandit"^^xsd:string,
        "Piero Bonatti"^^xsd:string ;
    dct:description "Processing that involves use of innovative and new technologies"@en ;
    dct:source <https://eur-lex.europa.eu/eli/reg/2016/679/art_4/par_2/oj> ;
    rdfs:isDefinedBy dpvo: ;
    rdfs:subClassOf dpvo:ProcessingContext ;
    sw:term_status "accepted"@en .

dpvo:InternalResourceOptimisation a owl:Class ;
    rdfs:label "Internal Resource Optimisation"@en ;
    dct:created "2019-04-05"^^xsd:date ;
    dct:creator "Axel Polleres"^^xsd:string,
        "Elmar Kiesling"^^xsd:string,
        "Fajar Ekaputra"^^xsd:string,
        "Harshvardhan J. Pandit"^^xsd:string,
        "Javier Fernandez"^^xsd:string,
        "Simon Steyskal"^^xsd:string ;
    dct:description "Purposes associated with optimisation of internal resource availability and usage for organisation"@en ;
    rdfs:isDefinedBy dpvo: ;
    rdfs:subClassOf dpvo:OptimisationForController ;
    sw:term_status "accepted"@en .

dpvo:InternationalOrganisation a owl:Class ;
    rdfs:label "International Organisation"@en ;
    dct:created "2022-03-23"^^xsd:date ;
    dct:creator "Georg P. Krog"^^xsd:string,
        "Julian Flake"^^xsd:string ;
    dct:description "An organisation and its subordinate bodies governed by public international law, or any other body which is set up by, or on the basis of, an agreement between two or more countries"@en ;
    dct:modified "2020-10-05"^^xsd:date ;
    dct:source <https://eur-lex.europa.eu/eli/reg/2016/679/art_4/par_26/oj> ;
    rdfs:isDefinedBy dpvo: ;
    rdfs:subClassOf dpvo:Organisation ;
    sw:term_status "modified"@en .

dpvo:IntrusionDetectionSystem a owl:Class ;
    rdfs:label "Intrusion Detection System"@en ;
    dct:created "2022-08-17"^^xsd:date ;
    dct:creator "Harshvardhan J. Pandit"^^xsd:string ;
    dct:description "Use of measures to detect intrusions and other unauthorised attempts to gain access to a system"@en ;
    dct:source <https://www.enisa.europa.eu/publications/reference-incident-classification-taxonomy/> ;
    rdfs:isDefinedBy dpvo: ;
    rdfs:subClassOf dpvo:SecurityMethod ;
    sw:term_status "accepted"@en .

dpvo:JobApplicant a owl:Class ;
    rdfs:label "Job Applicant"@en ;
    dct:created "2022-04-06"^^xsd:date ;
    dct:creator "Beatriz Esteves"^^xsd:string,
        "Georg P. Krog"^^xsd:string,
        "Harshvardhan J. Pandit"^^xsd:string,
        "Julian Flake"^^xsd:string,
        "Paul Ryan"^^xsd:string ;
    dct:description "Data subjects that apply for jobs or employments"@en ;
    rdfs:isDefinedBy dpvo: ;
    rdfs:subClassOf dpvo:Applicant ;
    sw:term_status "accepted"@en .

dpvo:JointDataControllersAgreement a owl:Class ;
    rdfs:label "Joint Data Controllers Agreement"@en ;
    dct:created "2022-01-26"^^xsd:date ;
    dct:creator "Beatriz Esteves"^^xsd:string,
        "Georg P Krog"^^xsd:string,
        "Harshvardhan J. Pandit"^^xsd:string,
        "Julian Flake"^^xsd:string,
        "Paul Ryan"^^xsd:string ;
    dct:description "An agreement outlining conditions, criteria, obligations, responsibilities, and specifics for carrying out processing of personal data between Controllers within a Joint Controllers relationship"@en ;
    rdfs:isDefinedBy dpvo: ;
    rdfs:subClassOf dpvo:DataProcessingAgreement ;
    sw:term_status "accepted"@en .

dpvo:LargeDataVolume a owl:NamedIndividual,
        dpvo:DataVolume ;
    rdfs:label "Large Data Volume"@en ;
    dct:created "2022-06-15"^^xsd:date ;
    dct:creator "Harshvardhan J. Pandit"^^xsd:string ;
    dct:description "Data volume that is considered large within the context"@en ;
    rdfs:isDefinedBy dpvo: ;
    sw:term_status "accepted"@en .

dpvo:LargeScaleOfDataSubjects a owl:NamedIndividual,
        dpvo:DataSubjectScale ;
    rdfs:label "Large Scale Of Data Subjects"@en ;
    dct:created "2022-06-15"^^xsd:date ;
    dct:creator "Harshvardhan J. Pandit"^^xsd:string ;
    dct:description "Scale of data subjects considered large within the context"@en ;
    rdfs:isDefinedBy dpvo: ;
    sw:term_status "accepted"@en .

dpvo:LargeScaleProcessing a owl:NamedIndividual,
        dpvo:ProcessingScale ;
    rdfs:label "Large Scale Processing"@en ;
    dct:created "2020-11-04"^^xsd:date ;
    dct:creator "Harshvardhan J. Pandit"^^xsd:string,
        "Piero Bonatti"^^xsd:string ;
    dct:description "Processing that takes place at large scales (as specified by some criteria)"@en ;
    dct:modified "2022-09-07"^^xsd:date ;
    dct:source <https://eur-lex.europa.eu/eli/reg/2016/679/art_4/par_2/oj> ;
    rdfs:comment "The exact definition of what constitutes \"large scale\" depends on use of jurisdictional, domain-specific, or other forms of externally defined criterias. Where possible, this should be reflected by extending this term with the appropriate context."@en ;
    rdfs:isDefinedBy dpvo: ;
    sw:term_status "modified"@en .

dpvo:Lawful a owl:NamedIndividual,
        dpvo:Lawfulness ;
    rdfs:label "Lawful"@en ;
    dct:created "2022-10-19"^^xsd:date ;
    dct:creator "Harshvardhan J. Pandit"^^xsd:string ;
    dct:description "State of being lawful or legally compliant"@en ;
    rdfs:isDefinedBy dpvo: ;
    sw:term_status "accepted"@en .

dpvo:LawfulnessUnkown a owl:NamedIndividual,
        dpvo:Lawfulness ;
    rdfs:label "Lawfulness Unknown"@en ;
    dct:created "2022-10-19"^^xsd:date ;
    dct:creator "Harshvardhan J. Pandit"^^xsd:string ;
    dct:description "State of the lawfulness not being known"@en ;
    rdfs:isDefinedBy dpvo: ;
    sw:term_status "accepted"@en .

dpvo:LegalCompliance a owl:Class ;
    rdfs:label "Legal Compliance"@en ;
    dct:created "2020-11-04"^^xsd:date ;
    dct:creator "Beatriz Esteves"^^xsd:string,
        "Georg P Krog"^^xsd:string,
        "Harshvardhan J. Pandit"^^xsd:string ;
    dct:description "Purposes associated with carrying out data processing to fulfill a legal or statutory obligation"@en ;
    dct:modified "2022-11-09"^^xsd:date ;
    rdfs:comment "This purpose only refers to processing that is additionally required in order to fulfill the obligations and requirements associated with a law. For example, the use of consent would have its own separate purposes, with this purpose addressing a legal requirement for maintaining consent record (along with RecordManagement). This purpose will typically be used with Legal Obligation as the legal basis."@en ;
    rdfs:isDefinedBy dpvo: ;
    rdfs:subClassOf dpvo:FulfilmentOfObligation ;
    sw:term_status "accepted"@en .

dpvo:LegalObligation a owl:Class ;
    rdfs:label "Legal Obligation"@en ;
    dct:created "2021-04-07"^^xsd:date ;
    dct:creator "Harshvardhan J. Pandit"^^xsd:string ;
    dct:description "Legal Obligation to conduct the specified processing"@en ;
    rdfs:isDefinedBy dpvo: ;
    rdfs:subClassOf dpvo:LegalBasis ;
    sw:term_status "accepted"@en .

dpvo:LegitimateInterestAssessment a owl:Class ;
    rdfs:label "Legitimate Interest Assessment"@en ;
    dct:created "2021-09-08"^^xsd:date ;
    dct:creator "Georg P Krog"^^xsd:string,
        "Harshvardhan J. Pandit"^^xsd:string,
        "Paul Ryan"^^xsd:string ;
    dct:description "Indicates an assessment regarding the use of legitimate interest as a lawful basis by the data controller"@en ;
    rdfs:isDefinedBy dpvo: ;
    rdfs:subClassOf dpvo:Assessment ;
    sw:term_status "accepted"@en .

dpvo:LegitimateInterestOfController a owl:Class ;
    rdfs:label "Legitimate Interest of Controller"@en ;
    dct:created "2021-05-19"^^xsd:date ;
    dct:creator "Georg P Krog"^^xsd:string,
        "Harshvardhan J. Pandit"^^xsd:string,
        "Paul Ryan"^^xsd:string ;
    dct:description "Legitimate Interests of a Data Controller in conducting specified processing"@en ;
    rdfs:isDefinedBy dpvo: ;
    rdfs:subClassOf dpvo:LegitimateInterest ;
    sw:term_status "accepted"@en .

dpvo:LegitimateInterestOfDataSubject a owl:Class ;
    rdfs:label "Legitimate Interest of Data Subject"@en ;
    dct:created "2022-10-22"^^xsd:date ;
    dct:creator "Georg P Krog"^^xsd:string ;
    dct:description "Legitimate Interests of the Data Subject in conducting specified processing"@en ;
    rdfs:isDefinedBy dpvo: ;
    rdfs:subClassOf dpvo:LegitimateInterest ;
    sw:term_status "accepted"@en .

dpvo:LegitimateInterestOfThirdParty a owl:Class ;
    rdfs:label "Legitimate Interest of Third Party"@en ;
    dct:created "2021-05-19"^^xsd:date ;
    dct:creator "Georg P Krog"^^xsd:string,
        "Harshvardhan J. Pandit"^^xsd:string,
        "Paul Ryan"^^xsd:string ;
    dct:description "Legitimate Interests of a Third Party in conducting specified processing"@en ;
    rdfs:isDefinedBy dpvo: ;
    rdfs:subClassOf dpvo:LegitimateInterest ;
    sw:term_status "accepted"@en .

dpvo:LocalEnvironmentScale a owl:NamedIndividual,
        dpvo:GeographicCoverage ;
    rdfs:label "Local Environment Scale"@en ;
    dct:created "2022-06-15"^^xsd:date ;
    dct:creator "Harshvardhan J. Pandit"^^xsd:string ;
    dct:description "Geographic coverage spanning a specific environment within the locality"@en ;
    rdfs:comment "For example, geographic scale of an event take place in a specific building or room"@en ;
    rdfs:isDefinedBy dpvo: ;
    sw:term_status "accepted"@en .

dpvo:LocalityScale a owl:NamedIndividual,
        dpvo:GeographicCoverage ;
    rdfs:label "Locality Scale"@en ;
    dct:created "2022-06-15"^^xsd:date ;
    dct:creator "Harshvardhan J. Pandit"^^xsd:string ;
    dct:description "Geographic coverage spanning a specific locality"@en ;
    rdfs:comment "For example, geographic scale of a city or an area within a city"@en ;
    rdfs:isDefinedBy dpvo: ;
    sw:term_status "accepted"@en .

dpvo:LoggingPolicies a owl:Class ;
    rdfs:label "Logging Policies"@en ;
    dct:created "2022-08-17"^^xsd:date ;
    dct:creator "Harshvardhan J. Pandit"^^xsd:string ;
    dct:description "Policy for logging of information"@en ;
    dct:source <https://www.enisa.europa.eu/publications/5g-cybersecurity-standards> ;
    rdfs:isDefinedBy dpvo: ;
    rdfs:subClassOf dpvo:GovernanceProcedures ;
    sw:term_status "accepted"@en .

dpvo:MaintainCreditCheckingDatabase a owl:Class ;
    rdfs:label "Maintain Credit Checking Database"@en ;
    dct:created "2022-06-15"^^xsd:date ;
    dct:creator "Georg P Krog"^^xsd:string,
        "Harshvardhan J. Pandit"^^xsd:string ;
    dct:description "Purposes associated with maintaining a Credit Checking Database"@en ;
    rdfs:isDefinedBy dpvo: ;
    rdfs:subClassOf dpvo:CreditChecking ;
    sw:term_status "accepted"@en .

dpvo:MaintainCreditRatingDatabase a owl:Class ;
    rdfs:label "Maintain Credit Rating Database"@en ;
    dct:created "2022-06-15"^^xsd:date ;
    dct:creator "Georg P Krog"^^xsd:string,
        "Harshvardhan J. Pandit"^^xsd:string ;
    dct:description "Purposes associated with maintaining a Credit Rating Database"@en ;
    rdfs:isDefinedBy dpvo: ;
    rdfs:subClassOf dpvo:CreditChecking ;
    sw:term_status "accepted"@en .

dpvo:MaintainFraudDatabase a owl:Class ;
    rdfs:label "MaintainFraudDatabase"@en ;
    dct:created "2022-06-15"^^xsd:date ;
    dct:creator "Georg P Krog"^^xsd:string,
        "Harshvardhan J. Pandit"^^xsd:string ;
    dct:description "Purposes associated with maintaining a database related to identifying and identified fraud risks and fraud incidents"@en ;
    rdfs:isDefinedBy dpvo: ;
    rdfs:subClassOf dpvo:FraudPreventionAndDetection ;
    sw:term_status "accepted"@en .

dpvo:MakeAvailable a owl:Class ;
    rdfs:label "Make Available"@en ;
    dct:created "2019-05-07"^^xsd:date ;
    dct:description "to transform or publish data to be used"@en ;
    dct:source <https://eur-lex.europa.eu/eli/reg/2016/679/art_4/par_2/oj> ;
    rdfs:isDefinedBy dpvo: ;
    rdfs:subClassOf dpvo:Disclose ;
    sw:term_status "accepted"@en .

dpvo:Match a owl:Class ;
    rdfs:label "Match"@en ;
    dct:created "2022-04-20"^^xsd:date ;
    dct:creator "Harshvardhan J. Pandit"^^xsd:string ;
    dct:description "to combine, compare, or match data from different sources"@en ;
    dct:source <https://ec.europa.eu/newsroom/article29/items/611236> ;
    rdfs:isDefinedBy dpvo: ;
    rdfs:subClassOf dpvo:Use ;
    sw:term_status "accepted"@en .

dpvo:MaterialDamage a owl:Class ;
    rdfs:label "Material Damage"@en ;
    dct:created "2022-03-30"^^xsd:date ;
    dct:creator "Harshvardhan J. Pandit"^^xsd:string ;
    dct:description "Impact that acts as or causes material damages"@en ;
    rdfs:isDefinedBy dpvo: ;
    rdfs:subClassOf dpvo:Damage ;
    sw:term_status "accepted"@en .

dpvo:MediumDataVolume a owl:NamedIndividual,
        dpvo:DataVolume ;
    rdfs:label "Medium Data Volume"@en ;
    dct:created "2022-06-15"^^xsd:date ;
    dct:creator "Georg P Krog"^^xsd:string,
        "Harshvardhan J. Pandit"^^xsd:string,
        "Paul Ryan"^^xsd:string ;
    dct:description "Data volume that is considered medium i.e. neither large nor small within the context"@en ;
    rdfs:isDefinedBy dpvo: ;
    sw:term_status "accepted"@en .

dpvo:MediumScaleOfDataSubjects a owl:NamedIndividual,
        dpvo:DataSubjectScale ;
    rdfs:label "Medium Scale Of Data Subjects"@en ;
    dct:created "2022-06-15"^^xsd:date ;
    dct:creator "Georg P Krog"^^xsd:string,
        "Harshvardhan J. Pandit"^^xsd:string,
        "Paul Ryan"^^xsd:string ;
    dct:description "Scale of data subjects considered medium i.e. neither large nor small within the context"@en ;
    rdfs:isDefinedBy dpvo: ;
    sw:term_status "accepted"@en .

dpvo:MediumScaleProcessing a owl:NamedIndividual,
        dpvo:ProcessingScale ;
    rdfs:label "Medium Scale Processing"@en ;
    dct:created "2022-09-07"^^xsd:date ;
    dct:creator "Harshvardhan J. Pandit"^^xsd:string ;
    dct:description "Processing that takes place at medium scales (as specified by some criteria)"@en ;
    rdfs:isDefinedBy dpvo: ;
    sw:term_status "accepted"@en .

dpvo:Member a owl:Class ;
    rdfs:label "Member"@en ;
    dct:created "2022-04-06"^^xsd:date ;
    dct:creator "Beatriz Esteves"^^xsd:string,
        "Georg P. Krog"^^xsd:string,
        "Harshvardhan J. Pandit"^^xsd:string,
        "Julian Flake"^^xsd:string,
        "Paul Ryan"^^xsd:string ;
    dct:description "Data subjects that are members of a group, organisation, or other collectives"@en ;
    rdfs:isDefinedBy dpvo: ;
    rdfs:subClassOf dpvo:DataSubject ;
    sw:term_status "accepted"@en .

dpvo:MemberPartnerManagement a owl:Class ;
    rdfs:label "Members and Partners Management"@en ;
    dct:created "2021-09-01"^^xsd:date ;
    dct:creator "David Hickey"^^xsd:string,
        "Georg P Krog"^^xsd:string,
        "Harshvardhan J. Pandit"^^xsd:string,
        "Paul Ryan"^^xsd:string ;
    dct:description "Purposes associated with maintaining a registry of shareholders, members, or partners for governance, administration, and management functions"@en ;
    dct:source <https://www.privacycommission.be/nl/model-voor-een-register-van-de-verwerkingsactiviteiten> ;
    rdfs:isDefinedBy dpvo: ;
    rdfs:subClassOf dpvo:OrganisationGovernance ;
    sw:term_status "accepted"@en .

dpvo:MentallyVulnerableDataSubject a owl:Class ;
    rdfs:label "Mentally Vulnerable Data Subject"@en ;
    dct:created "2022-06-15"^^xsd:date ;
    dct:creator "Georg P Krog"^^xsd:string ;
    dct:description "Data subjects that are considered mentally vulnerable"@en ;
    rdfs:isDefinedBy dpvo: ;
    rdfs:subClassOf dpvo:VulnerableDataSubject ;
    sw:term_status "accepted"@en .

dpvo:MessageAuthenticationCodes a owl:Class ;
    rdfs:label "Message Authentication Codes (MAC)"@en ;
    dct:created "2022-08-17"^^xsd:date ;
    dct:creator "Harshvardhan J. Pandit"^^xsd:string ;
    dct:description "Use of cryptographic methods to authenticate messages"@en ;
    dct:source <https://www.enisa.europa.eu/publications/reference-incident-classification-taxonomy/> ;
    rdfs:isDefinedBy dpvo: ;
    rdfs:subClassOf dpvo:CryptographicAuthentication ;
    sw:term_status "accepted"@en .

dpvo:MobilePlatformSecurity a owl:Class ;
    rdfs:label "Mobile Platform Security"@en ;
    dct:created "2022-08-17"^^xsd:date ;
    dct:creator "Harshvardhan J. Pandit"^^xsd:string ;
    dct:description "Security implemented over a mobile platform"@en ;
    dct:source <https://www.enisa.europa.eu/publications/reference-incident-classification-taxonomy/> ;
    rdfs:isDefinedBy dpvo: ;
    rdfs:subClassOf dpvo:SecurityMethod ;
    sw:term_status "accepted"@en .

dpvo:Modify a owl:Class ;
    rdfs:label "Modify"@en ;
    dct:created "2022-06-15"^^xsd:date ;
    dct:creator "Georg P Krog"^^xsd:string,
        "Harshvardhan J. Pandit"^^xsd:string ;
    dct:description "to modify or change data"@en ;
    rdfs:isDefinedBy dpvo: ;
    rdfs:subClassOf dpvo:Alter ;
    sw:term_status "accepted"@en .

dpvo:Monitor a owl:Class ;
    rdfs:label "Monitor"@en ;
    dct:created "2022-06-15"^^xsd:date ;
    dct:creator "Georg P Krog"^^xsd:string,
        "Harshvardhan J. Pandit"^^xsd:string ;
    dct:description "to monitor data for some criteria"@en ;
    rdfs:isDefinedBy dpvo: ;
    rdfs:subClassOf dpvo:Consult ;
    sw:term_status "accepted"@en .

dpvo:MonitoringPolicies a owl:Class ;
    rdfs:label "Monitoring Policies"@en ;
    dct:created "2022-08-17"^^xsd:date ;
    dct:creator "Harshvardhan J. Pandit"^^xsd:string ;
    dct:description "Policy for monitoring (e.g. progress, performance)"@en ;
    dct:source <https://www.enisa.europa.eu/publications/5g-cybersecurity-standards> ;
    rdfs:isDefinedBy dpvo: ;
    rdfs:subClassOf dpvo:GovernanceProcedures ;
    sw:term_status "accepted"@en .

dpvo:MonotonicCounterPseudonymisation a owl:Class ;
    rdfs:label "Monotonic Counter Pseudonymisation"@en ;
    dct:created "2022-08-17"^^xsd:date ;
    dct:creator "Harshvardhan J. Pandit"^^xsd:string ;
    dct:description "A simple pseudonymisation method where identifiers are substituted by a number chosen by a monotonic counter"@en ;
    dct:modified "2022-10-13"^^xsd:date ;
    dct:source <https://www.enisa.europa.eu/publications/data-pseudonymisation-advanced-techniques-and-use-cases> ;
    rdfs:isDefinedBy dpvo: ;
    rdfs:subClassOf dpvo:Pseudonymisation ;
    sw:term_status "modified"@en .

dpvo:Move a owl:Class ;
    rdfs:label "Move"@en ;
    dct:created "2019-05-07"^^xsd:date ;
    dct:description "to move data from one location to another including deleting the original copy"@en ;
    dct:source <https://specialprivacy.ercim.eu/vocabs/processing> ;
    rdfs:isDefinedBy dpvo: ;
    rdfs:seeAlso svpr:Move ;
    rdfs:subClassOf dpvo:Transfer ;
    sw:term_status "accepted"@en .

dpvo:MultiFactorAuthentication a owl:Class ;
    rdfs:label "Multi-Factor Authentication (MFA)"@en ;
    dct:created "2022-08-17"^^xsd:date ;
    dct:creator "Harshvardhan J. Pandit"^^xsd:string ;
    dct:description "An authentication system that uses two or more methods to authenticate"@en ;
    dct:source <https://www.enisa.europa.eu/publications/reference-incident-classification-taxonomy/> ;
    rdfs:isDefinedBy dpvo: ;
    rdfs:subClassOf dpvo:AuthenticationProtocols ;
    sw:term_status "accepted"@en .

dpvo:MultiNationalScale a owl:NamedIndividual,
        dpvo:GeographicCoverage ;
    rdfs:label "Multi National Scale"@en ;
    dct:created "2022-06-15"^^xsd:date ;
    dct:creator "Harshvardhan J. Pandit"^^xsd:string ;
    dct:description "Geographic coverage spanning multiple nations"@en ;
    rdfs:isDefinedBy dpvo: ;
    sw:term_status "accepted"@en .

dpvo:NDA a owl:Class ;
    rdfs:label "Non-Disclosure Agreement (NDA)"@en ;
    dct:created "2019-04-05"^^xsd:date ;
    dct:creator "Axel Polleres"^^xsd:string,
        "Harshvardhan J. Pandit"^^xsd:string,
        "Mark Lizar"^^xsd:string,
        "Rob Brennan"^^xsd:string ;
    dct:description "Non-disclosure Agreements e.g. preserving confidentiality of information"@en ;
    rdfs:isDefinedBy dpvo: ;
    rdfs:subClassOf dpvo:LegalAgreement ;
    sw:term_status "accepted"@en .

dpvo:NationalAuthority a owl:Class ;
    rdfs:label "National Authority"@en ;
    dct:created "2022-02-02"^^xsd:date ;
    dct:creator "Harshvardhan J. Pandit"^^xsd:string ;
    dct:description "An authority tasked with overseeing legal compliance for a nation"@en ;
    dct:source <http://purl.org/adms> ;
    rdfs:isDefinedBy dpvo: ;
    rdfs:subClassOf dpvo:Authority ;
    sw:term_status "accepted"@en .

dpvo:NationalScale a owl:NamedIndividual,
        dpvo:GeographicCoverage ;
    rdfs:label "National Scale"@en ;
    dct:created "2022-06-15"^^xsd:date ;
    dct:creator "Harshvardhan J. Pandit"^^xsd:string ;
    dct:description "Geographic coverage spanning a nation"@en ;
    rdfs:isDefinedBy dpvo: ;
    sw:term_status "accepted"@en .

dpvo:NearlyGlobalScale a owl:NamedIndividual,
        dpvo:GeographicCoverage ;
    rdfs:label "Nearly Global Scale"@en ;
    dct:created "2022-06-15"^^xsd:date ;
    dct:creator "Harshvardhan J. Pandit"^^xsd:string ;
    dct:description "Geographic coverage nearly spanning the entire globe"@en ;
    rdfs:isDefinedBy dpvo: ;
    sw:term_status "accepted"@en .

dpvo:NetworkProxyRouting a owl:Class ;
    rdfs:label "Network Proxy Routing"@en ;
    dct:created "2022-08-17"^^xsd:date ;
    dct:creator "Harshvardhan J. Pandit"^^xsd:string ;
    dct:description "Use of network routing using proxy"@en ;
    dct:source <https://www.enisa.europa.eu/publications/data-protection-engineering> ;
    rdfs:isDefinedBy dpvo: ;
    rdfs:subClassOf dpvo:SecurityMethod ;
    sw:term_status "accepted"@en .

dpvo:NetworkSecurityProtocols a owl:Class ;
    rdfs:label "Network Security Protocols"@en ;
    dct:created "2022-08-17"^^xsd:date ;
    dct:creator "Harshvardhan J. Pandit"^^xsd:string ;
    dct:description "Security implemented at or over networks protocols"@en ;
    dct:source <https://www.enisa.europa.eu/publications/reference-incident-classification-taxonomy/> ;
    rdfs:isDefinedBy dpvo: ;
    rdfs:subClassOf dpvo:SecurityMethod ;
    sw:term_status "accepted"@en .

dpvo:NonCitizen a owl:Class ;
    rdfs:label "Non-Citizen"@en ;
    dct:created "2022-04-06"^^xsd:date ;
    dct:creator "Beatriz Esteves"^^xsd:string,
        "Georg P. Krog"^^xsd:string,
        "Harshvardhan J. Pandit"^^xsd:string,
        "Julian Flake"^^xsd:string,
        "Paul Ryan"^^xsd:string ;
    dct:description "Data subjects that are not citizens (for a jurisdiction)"@en ;
    rdfs:isDefinedBy dpvo: ;
    rdfs:subClassOf dpvo:DataSubject ;
    sw:term_status "accepted"@en .

dpvo:NonCommercialResearch a owl:Class ;
    rdfs:label "Non-Commercial Research"@en ;
    dct:created "2019-04-05"^^xsd:date ;
    dct:creator "Axel Polleres"^^xsd:string,
        "Elmar Kiesling"^^xsd:string,
        "Fajar Ekaputra"^^xsd:string,
        "Harshvardhan J. Pandit"^^xsd:string,
        "Javier Fernandez"^^xsd:string,
        "Simon Steyskal"^^xsd:string ;
    dct:description "Purposes associated with conducting research in a non-commercial setting e.g. for a non-profit-organisation (NGO)"@en ;
    rdfs:isDefinedBy dpvo: ;
    rdfs:subClassOf dpvo:ResearchAndDevelopment ;
    sw:term_status "accepted"@en .

dpvo:NonCompliant a owl:NamedIndividual,
        dpvo:ComplianceStatus ;
    rdfs:label "Non Compliant"@en ;
    dct:created "2022-05-18"^^xsd:date ;
    dct:creator "Harshvardhan J. Pandit"^^xsd:string ;
    dct:description "State of non-compliance where objectives have not been met, but have not been violated"@en ;
    dct:modified "2022-09-07"^^xsd:date ;
    rdfs:comment "Changed from not compliant for consistency in commonly used terms"@en ;
    rdfs:isDefinedBy dpvo: ;
    sw:term_status "changed"@en .

dpvo:NonConformant a owl:NamedIndividual,
        dpvo:ConformanceStatus ;
    rdfs:label "NonConformant"@en ;
    dct:created "2022-10-22"^^xsd:date ;
    dct:creator "Harshvardhan J. Pandit"^^xsd:string ;
    dct:description "State of being non-conformant"@en ;
    rdfs:isDefinedBy dpvo: ;
    sw:term_status "accepted"@en .

dpvo:NonGovernmentalOrganisation a owl:Class ;
    rdfs:label "Non-Governmental Organisation"@en ;
    dct:created "2022-02-02"^^xsd:date ;
    dct:creator "Harshvardhan J. Pandit"^^xsd:string ;
    dct:description "An organisation not part of or independent from the government"@en ;
    dct:modified "2020-10-05"^^xsd:date ;
    dct:source <http://purl.org/adms> ;
    rdfs:isDefinedBy dpvo: ;
    rdfs:subClassOf dpvo:Organisation ;
    sw:term_status "modified"@en .

dpvo:NonMaterialDamage a owl:Class ;
    rdfs:label "Non-Material Damage"@en ;
    dct:created "2022-03-30"^^xsd:date ;
    dct:creator "Harshvardhan J. Pandit"^^xsd:string ;
    dct:description "Impact that acts as or causes non-material damages"@en ;
    rdfs:isDefinedBy dpvo: ;
    rdfs:subClassOf dpvo:Damage ;
    sw:term_status "accepted"@en .

dpvo:NonProfitOrganisation a owl:Class ;
    rdfs:label "Non-Profit Organisation"@en ;
    dct:created "2022-02-02"^^xsd:date ;
    dct:creator "Harshvardhan J. Pandit"^^xsd:string ;
    dct:description "An organisation that does not aim to achieve profit as its primary goal"@en ;
    dct:modified "2020-10-05"^^xsd:date ;
    dct:source <http://purl.org/adms> ;
    rdfs:isDefinedBy dpvo: ;
    rdfs:subClassOf dpvo:Organisation ;
    sw:term_status "modified"@en .

dpvo:NonPublicDataSource a owl:NamedIndividual,
        dpvo:DataSource ;
    rdfs:label "Non-Public Data Source"@en ;
    dct:created "2022-01-26"^^xsd:date ;
    dct:creator "Beatriz Esteves"^^xsd:string,
        "Georg P Krog"^^xsd:string,
        "Harshvardhan J. Pandit"^^xsd:string,
        "Julian Flake"^^xsd:string,
        "Paul Ryan"^^xsd:string ;
    dct:description "A source of data that is not publicly accessible or available"@en ;
    rdfs:isDefinedBy dpvo: ;
    sw:term_status "accepted"@en .

dpvo:NotRequired a owl:NamedIndividual,
        dpvo:Necessity ;
    rdfs:label "Not Required"@en ;
    dct:created "2022-02-15"^^xsd:date ;
    dct:creator "Beatriz Esteves"^^xsd:string,
        "Georg P Krog"^^xsd:string,
        "Harshvardhan J. Pandit"^^xsd:string,
        "Julian Flake"^^xsd:string,
        "Paul Ryan"^^xsd:string ;
    dct:description "Indication of neither being required nor optional i.e. not relevant or needed"@en ;
    rdfs:isDefinedBy dpvo: ;
    sw:term_status "accepted"@en .

dpvo:Observe a owl:Class ;
    rdfs:label "Observe"@en ;
    dct:created "2022-06-15"^^xsd:date ;
    dct:creator "Georg P Krog"^^xsd:string,
        "Harshvardhan J. Pandit"^^xsd:string ;
    dct:description "to obtain data through observation"@en ;
    rdfs:isDefinedBy dpvo: ;
    rdfs:subClassOf dpvo:Obtain ;
    sw:term_status "accepted"@en .

dpvo:ObservedPersonalData a owl:Class ;
    rdfs:label "Observed Personal Data"@en ;
    dct:created "2022-08-24"^^xsd:date ;
    dct:creator "Georg P Krog"^^xsd:string ;
    dct:description "Personal Data that has been collected through observation of the Data Subject(s)"@en ;
    rdfs:isDefinedBy dpvo: ;
    rdfs:subClassOf dpvo:CollectedPersonalData ;
    sw:term_status "accepted"@en .

dpvo:OfficialAuthorityOfController a owl:Class ;
    rdfs:label "Official Authority of Controller"@en ;
    dct:created "2021-05-05"^^xsd:date ;
    dct:creator "Georg P Krog"^^xsd:string,
        "Harshvardhan J. Pandit"^^xsd:string,
        "Paul Ryan"^^xsd:string ;
    dct:description "Processing necessary or authorised through the official authority granted to or vested in the Data Controller"@en ;
    rdfs:isDefinedBy dpvo: ;
    rdfs:subClassOf dpvo:LegalBasis ;
    sw:term_status "accepted"@en .

dpvo:OftenFrequency a owl:Class ;
    rdfs:label "Often Frequency"@en ;
    dct:created "2022-06-15"^^xsd:date ;
    dct:creator "Harshvardhan J. Pandit"^^xsd:string ;
    dct:description "Frequency where occurences are often or frequent, but not continous"@en ;
    dct:modified "2020-10-05"^^xsd:date ;
    rdfs:isDefinedBy dpvo: ;
    rdfs:subClassOf dpvo:Frequency ;
    sw:term_status "modified"@en .

dpvo:OperatingSystemSecurity a owl:Class ;
    rdfs:label "Operating System Security"@en ;
    dct:created "2022-08-17"^^xsd:date ;
    dct:creator "Harshvardhan J. Pandit"^^xsd:string ;
    dct:description "Security implemented at or through operating systems"@en ;
    dct:source <https://www.enisa.europa.eu/publications/reference-incident-classification-taxonomy/> ;
    rdfs:isDefinedBy dpvo: ;
    rdfs:subClassOf dpvo:SecurityMethod ;
    sw:term_status "accepted"@en .

dpvo:OptimiseUserInterface a owl:Class ;
    rdfs:label "Optimise User Interface"@en ;
    dct:created "2019-04-05"^^xsd:date ;
    dct:creator "Axel Polleres"^^xsd:string,
        "Elmar Kiesling"^^xsd:string,
        "Fajar Ekaputra"^^xsd:string,
        "Harshvardhan J. Pandit"^^xsd:string,
        "Javier Fernandez"^^xsd:string,
        "Simon Steyskal"^^xsd:string ;
    dct:description "Purposes associated with optimisation of interfaces presented to the user"@en ;
    rdfs:isDefinedBy dpvo: ;
    rdfs:subClassOf dpvo:OptimisationForConsumer ;
    sw:term_status "accepted"@en .

dpvo:Optional a owl:NamedIndividual,
        dpvo:Necessity ;
    rdfs:label "Optional"@en ;
    dct:created "2022-02-14"^^xsd:date ;
    dct:creator "Beatriz Esteves"^^xsd:string,
        "Georg P Krog"^^xsd:string,
        "Harshvardhan J. Pandit"^^xsd:string,
        "Julian Flake"^^xsd:string,
        "Paul Ryan"^^xsd:string ;
    dct:description "Indication of 'optional' or 'voluntary'"@en ;
    rdfs:isDefinedBy dpvo: ;
    sw:term_status "accepted"@en .

dpvo:OrganisationComplianceManagement a owl:Class ;
    rdfs:label "Organisation Compliance Management"@en ;
    dct:created "2021-09-01"^^xsd:date ;
    dct:creator "David Hickey"^^xsd:string,
        "Georg P Krog"^^xsd:string,
        "Harshvardhan J. Pandit"^^xsd:string,
        "Paul Ryan"^^xsd:string ;
    dct:description "Purposes associated with managing compliance for organisation in relation to internal policies"@en ;
    rdfs:comment "Note that this concept relates to internal organisational compliance. The concept LegalCompliance should be used for external legal or regulatory compliance."@en ;
    rdfs:isDefinedBy dpvo: ;
    rdfs:subClassOf dpvo:OrganisationGovernance ;
    sw:term_status "accepted"@en .

dpvo:OrganisationRiskManagement a owl:Class ;
    rdfs:label "Organisation Risk Management"@en ;
    dct:created "2021-09-01"^^xsd:date ;
    dct:creator "David Hickey"^^xsd:string,
        "Georg P Krog"^^xsd:string,
        "Harshvardhan J. Pandit"^^xsd:string,
        "Paul Ryan"^^xsd:string ;
    dct:description "Purposes associated with managing risk for organisation's activities"@en ;
    rdfs:isDefinedBy dpvo: ;
    rdfs:subClassOf dpvo:OrganisationGovernance ;
    sw:term_status "accepted"@en .

dpvo:OrganisationalUnit a owl:Class ;
    rdfs:label "Organisational Unit"@en ;
    dct:created "2022-03-23"^^xsd:date ;
    dct:creator "Harshvardhan J. Pandit"^^xsd:string,
        "Paul Ryan"^^xsd:string ;
    dct:description "Entity within an organisation that does not constitute as a separate legal entity"@en ;
    rdfs:isDefinedBy dpvo: ;
    rdfs:subClassOf dpvo:Entity ;
    sw:term_status "accepted"@en .

dpvo:PIA a owl:Class ;
    rdfs:label "Privacy Impact Assessment"@en ;
    dct:created "2020-11-04"^^xsd:date ;
    dct:creator "Georg P Krog"^^xsd:string,
        "Harshvardhan J. Pandit"^^xsd:string,
        "Paul Ryan"^^xsd:string ;
    dct:description "Carrying out an impact assessment regarding privacy risks"@en ;
    rdfs:isDefinedBy dpvo: ;
    rdfs:subClassOf dpvo:ImpactAssessment ;
    sw:term_status "accepted"@en .

dpvo:ParentOfDataSubject a owl:Class ;
    rdfs:label "Parent(s) of Data Subject"@en ;
    dct:created "2022-08-03"^^xsd:date ;
    dct:creator "Georg P Krog"^^xsd:string ;
    dct:description "Parent(s) of data subjects such as children"@en ;
    rdfs:isDefinedBy dpvo: ;
    rdfs:subClassOf dpvo:DataSubject ;
    sw:term_status "accepted"@en .

dpvo:PartiallyAutomatedProcessing a owl:NamedIndividual,
        dpvo:AutomationOfProcessing ;
    rdfs:label "Partially Automated Processing"@en ;
    dct:created "2022-06-15"^^xsd:date ;
    dct:creator "Harshvardhan J. Pandit"^^xsd:string ;
    dct:description "Processing that is partially automated or semi-automated"@en ;
    rdfs:comment "For example, a series of distinct processing operations that are automated individually or have some human involvement"@en ;
    rdfs:isDefinedBy dpvo: ;
    sw:term_status "accepted"@en .

dpvo:PartiallyCompliant a owl:NamedIndividual,
        dpvo:ComplianceStatus ;
    rdfs:label "Partially Compliant"@en ;
    dct:created "2022-05-18"^^xsd:date ;
    dct:creator "Harshvardhan J. Pandit"^^xsd:string ;
    dct:description "State of partially being compliant i.e. only some objectives have been met, and others have not been in violation"@en ;
    rdfs:isDefinedBy dpvo: ;
    sw:term_status "accepted"@en .

dpvo:Participant a owl:Class ;
    rdfs:label "Participant"@en ;
    dct:created "2022-04-06"^^xsd:date ;
    dct:creator "Beatriz Esteves"^^xsd:string,
        "Georg P. Krog"^^xsd:string,
        "Harshvardhan J. Pandit"^^xsd:string,
        "Julian Flake"^^xsd:string,
        "Paul Ryan"^^xsd:string ;
    dct:description "Data subjects that participate in some context such as volunteers in a function"@en ;
    rdfs:isDefinedBy dpvo: ;
    rdfs:subClassOf dpvo:DataSubject ;
    sw:term_status "accepted"@en .

dpvo:PassiveRight a owl:Class ;
    rdfs:label "Passive Right"@en ;
    dct:created "2022-10-22"^^xsd:date ;
    dct:creator "Beatriz Esteves"^^xsd:string,
        "Georg P Krog"^^xsd:string,
        "Harshvardhan J Pandit"^^xsd:string,
        "Paul Ryan"^^xsd:string ;
    dct:description "The right(s) applicable, provided, or expected that are always (passively) applicable"@en ;
    rdfs:comment "Passive rights do not require the entity to request or exercise them. They are considered to be always applicable. For example, the Right to Privacy (in EU) does not require an exercise for it to be fulfilled."@en ;
    rdfs:isDefinedBy dpvo: ;
    rdfs:subClassOf dpvo:Right ;
    sw:term_status "accepted"@en .

dpvo:PasswordAuthentication a owl:Class ;
    rdfs:label "Password Authentication"@en ;
    dct:created "2022-08-17"^^xsd:date ;
    dct:creator "Harshvardhan J. Pandit"^^xsd:string ;
    dct:description "Use of passwords to perform authentication"@en ;
    dct:source <https://www.enisa.europa.eu/publications/reference-incident-classification-taxonomy/> ;
    rdfs:isDefinedBy dpvo: ;
    rdfs:subClassOf dpvo:AuthenticationProtocols ;
    sw:term_status "accepted"@en .

dpvo:Patient a owl:Class ;
    rdfs:label "Patient"@en ;
    dct:created "2022-04-06"^^xsd:date ;
    dct:creator "Beatriz Esteves"^^xsd:string,
        "Georg P. Krog"^^xsd:string,
        "Harshvardhan J. Pandit"^^xsd:string,
        "Julian Flake"^^xsd:string,
        "Paul Ryan"^^xsd:string ;
    dct:description "Data subjects that receive medican attention, treatment, care, advice, or other health related services"@en ;
    rdfs:isDefinedBy dpvo: ;
    rdfs:subClassOf dpvo:DataSubject ;
    sw:term_status "accepted"@en .

dpvo:PaymentManagement a owl:Class ;
    rdfs:label "Payment Management"@en ;
    dct:created "2020-11-04"^^xsd:date ;
    dct:creator "Beatriz Esteves"^^xsd:string,
        "Georg P Krog"^^xsd:string,
        "Harshvardhan J. Pandit"^^xsd:string ;
    dct:description "Purposes associated with processing and managing payment in relation to service, including invoicing and records"@en ;
    rdfs:isDefinedBy dpvo: ;
    rdfs:subClassOf dpvo:ServiceProvision ;
    sw:term_status "accepted"@en .

dpvo:PenetrationTestingMethods a owl:Class ;
    rdfs:label "Penetration Testing Methods"@en ;
    dct:created "2022-08-17"^^xsd:date ;
    dct:creator "Harshvardhan J. Pandit"^^xsd:string ;
    dct:description "Use of penetration testing to identity weaknessess and vulnerabilities through simulations"@en ;
    dct:source <https://www.enisa.europa.eu/publications/reference-incident-classification-taxonomy/> ;
    rdfs:isDefinedBy dpvo: ;
    rdfs:subClassOf dpvo:SecurityMethod ;
    sw:term_status "accepted"@en .

dpvo:PersonalisedBenefits a owl:Class ;
    rdfs:label "Personalised Benefits"@en ;
    dct:created "2019-04-05"^^xsd:date ;
    dct:creator "Axel Polleres"^^xsd:string,
        "Elmar Kiesling"^^xsd:string,
        "Fajar Ekaputra"^^xsd:string,
        "Harshvardhan J. Pandit"^^xsd:string,
        "Javier Fernandez"^^xsd:string,
        "Simon Steyskal"^^xsd:string ;
    dct:description "Purposes associated with creating and providing personalised benefits for a service"@en ;
    rdfs:isDefinedBy dpvo: ;
    rdfs:subClassOf dpvo:ServicePersonalisation ;
    sw:term_status "accepted"@en .

dpvo:PersonnelHiring a owl:Class ;
    rdfs:label "Personnel Hiring"@en ;
    dct:created "2022-04-20"^^xsd:date ;
    dct:creator "Harshvardhan J. Pandit"^^xsd:string ;
    dct:description "Purposes associated with management and execution of hiring processes of personnel"@en ;
    rdfs:isDefinedBy dpvo: ;
    rdfs:subClassOf dpvo:PersonnelManagement ;
    sw:term_status "accepted"@en .

dpvo:PersonnelPayment a owl:Class ;
    rdfs:label "Personnel Payment"@en ;
    dct:created "2022-04-20"^^xsd:date ;
    dct:creator "Harshvardhan J. Pandit"^^xsd:string ;
    dct:description "Purposes associated with management and execution of payment of personnel"@en ;
    rdfs:isDefinedBy dpvo: ;
    rdfs:subClassOf dpvo:PersonnelManagement ;
    sw:term_status "accepted"@en .

dpvo:PhysicalAccessControlMethod a owl:Class ;
    rdfs:label "Physical Access Control Method"@en ;
    dct:created "2022-06-15"^^xsd:date ;
    dct:creator "Georg P Krog"^^xsd:string ;
    dct:description "Access control applied for physical access e.g. premises or equipement"@en ;
    rdfs:isDefinedBy dpvo: ;
    rdfs:subClassOf dpvo:AccessControlMethod ;
    sw:term_status "accepted"@en .

dpvo:PostQuantumCryptography a owl:Class ;
    rdfs:label "Post-Quantum Cryptography"@en ;
    dct:created "2022-08-17"^^xsd:date ;
    dct:creator "Harshvardhan J. Pandit"^^xsd:string ;
    dct:description "Use of algorithms that are intended to be secure against cryptanalytic attack by a quantum computer"@en ;
    dct:source <https://www.enisa.europa.eu/publications/reference-incident-classification-taxonomy/> ;
    rdfs:isDefinedBy dpvo: ;
    rdfs:subClassOf dpvo:CryptographicMethods ;
    sw:term_status "accepted"@en .

dpvo:PrimaryImportance a owl:NamedIndividual,
        dpvo:Importance ;
    rdfs:label "Primary Importance"@en ;
    dct:created "2022-02-10"^^xsd:date ;
    dct:creator "Beatriz Esteves"^^xsd:string,
        "Georg P Krog"^^xsd:string,
        "Harshvardhan J. Pandit"^^xsd:string,
        "Julian Flake"^^xsd:string,
        "Paul Ryan"^^xsd:string ;
    dct:description "Indication of 'primary' or 'main' or 'core' importance"@en ;
    rdfs:isDefinedBy dpvo: ;
    sw:term_status "accepted"@en .

dpvo:PrivacyByDefault a owl:Class ;
    rdfs:label "Privacy by Default"@en ;
    dct:created "2019-04-05"^^xsd:date ;
    dct:creator "Axel Polleres"^^xsd:string,
        "Harshvardhan J. Pandit"^^xsd:string,
        "Mark Lizar"^^xsd:string,
        "Rob Brennan"^^xsd:string ;
    dct:description "Practices regarding selecting appropriate data protection and privacy measures as the 'default' in an activity or service"@en ;
    rdfs:isDefinedBy dpvo: ;
    rdfs:subClassOf dpvo:GuidelinesPrinciple ;
    sw:term_status "accepted"@en .

dpvo:PrivacyByDesign a owl:Class ;
    rdfs:label "Privacy by Design"@en ;
    dct:created "2019-04-05"^^xsd:date ;
    dct:creator "Axel Polleres"^^xsd:string,
        "Harshvardhan J. Pandit"^^xsd:string,
        "Mark Lizar"^^xsd:string,
        "Rob Brennan"^^xsd:string ;
    dct:description "Practices regarding incorporating data protection and privacy in the design of information and services"@en ;
    rdfs:isDefinedBy dpvo: ;
    rdfs:subClassOf dpvo:OrganisationalMeasure ;
    sw:term_status "accepted"@en .

dpvo:PrivacyPreservingProtocol a owl:Class ;
    rdfs:label "Privacy Preserving Protocol"@en ;
    dct:created "2022-08-17"^^xsd:date ;
    dct:creator "Harshvardhan J. Pandit"^^xsd:string ;
    dct:description "Use of protocols designed with the intention of provided additional guarentees regarding privacy"@en ;
    dct:source <https://www.enisa.europa.eu/publications/reference-incident-classification-taxonomy/> ;
    rdfs:isDefinedBy dpvo: ;
    rdfs:subClassOf dpvo:CryptographicMethods ;
    sw:term_status "accepted"@en .

dpvo:PrivateInformationRetrieval a owl:Class ;
    rdfs:label "Private Information Retrieval"@en ;
    dct:created "2022-08-17"^^xsd:date ;
    dct:creator "Harshvardhan J. Pandit"^^xsd:string ;
    dct:description "Use of cryptographic methods to retrieve a record from a system without revealing which record is retrieved"@en ;
    dct:source <https://www.enisa.europa.eu/publications/data-protection-engineering> ;
    rdfs:isDefinedBy dpvo: ;
    rdfs:subClassOf dpvo:CryptographicMethods ;
    sw:term_status "accepted"@en .

dpvo:PrivateLocation a owl:Class ;
    rdfs:label "Private Location"@en ;
    dct:created "2022-10-22"^^xsd:date ;
    dct:creator "Harshvardhan J. Pandit"^^xsd:string ;
    dct:description "Location that is not or cannot be accessed by the public and is controlled as a private space"@en ;
    rdfs:isDefinedBy dpvo: ;
    rdfs:subClassOf dpvo:LocalLocation ;
    sw:term_status "accepted"@en .

dpvo:ProfessionalTraining a owl:Class ;
    rdfs:label "Professional Training"@en ;
    dct:created "2022-08-17"^^xsd:date ;
    dct:creator "Harshvardhan J. Pandit"^^xsd:string ;
    dct:description "Training methods that are intended to provide professional knowledge and expertise"@en ;
    dct:source <https://www.enisa.europa.eu/publications/reference-incident-classification-taxonomy/> ;
    rdfs:isDefinedBy dpvo: ;
    rdfs:subClassOf dpvo:StaffTraining ;
    sw:term_status "accepted"@en .

dpvo:Profiling a owl:Class ;
    rdfs:label "Profiling"@en ;
    dct:created "2019-05-07"^^xsd:date ;
    dct:description "to create a profile that describes or represents a person"@en ;
    dct:source <https://eur-lex.europa.eu/eli/reg/2016/679/art_4/par_2/oj> ;
    rdfs:isDefinedBy dpvo: ;
    rdfs:subClassOf dpvo:Use ;
    sw:term_status "accepted"@en .

dpvo:ProvideEventRecommendations a owl:Class ;
    rdfs:label "Provide Event Recommendations"@en ;
    dct:created "2019-11-26"^^xsd:date ;
    dct:creator "Harshvardhan J. Pandit"^^xsd:string,
        "Rudy Jacob"^^xsd:string ;
    dct:description "Purposes associated with creating and providing personalised recommendations for events"@en ;
    dct:modified "2022-10-14"^^xsd:date ;
    dct:source <https://specialprivacy.ercim.eu/> ;
    rdfs:isDefinedBy dpvo: ;
    rdfs:subClassOf dpvo:ProvidePersonalisedRecommendations ;
    sw:term_status "accepted"@en .

dpvo:ProvideProductRecommendations a owl:Class ;
    rdfs:label "Provide Product Recommendations"@en ;
    dct:created "2019-04-05"^^xsd:date ;
    dct:creator "Axel Polleres"^^xsd:string,
        "Elmar Kiesling"^^xsd:string,
        "Fajar Ekaputra"^^xsd:string,
        "Harshvardhan J. Pandit"^^xsd:string,
        "Javier Fernandez"^^xsd:string,
        "Simon Steyskal"^^xsd:string ;
    dct:description "Purposes associated with creating and providing product recommendations e.g. suggest similar products"@en ;
    dct:modified "2022-10-14"^^xsd:date ;
    rdfs:isDefinedBy dpvo: ;
    rdfs:seeAlso svpu:Marketing ;
    rdfs:subClassOf dpvo:ProvidePersonalisedRecommendations ;
    sw:term_status "accepted"@en .

dpvo:Pseudonymise a owl:Class ;
    rdfs:label "Pseudonymise"@en ;
    dct:created "2019-05-07"^^xsd:date ;
    dct:creator "2022-10-14"^^xsd:string ;
    dct:description "to replace personal identifiable information by artificial identifiers"@en ;
    dct:source <https://eur-lex.europa.eu/eli/reg/2016/679/art_4/par_2/oj> ;
    rdfs:isDefinedBy dpvo: ;
    rdfs:subClassOf dpvo:Transform ;
    sw:term_status "modified"@en .

dpvo:PseudonymisedData a owl:Class ;
    rdfs:label "Pseudonymised Data"@en ;
    dct:created "2022-01-19"^^xsd:date ;
    dct:creator "Harshvardhan J. Pandit"^^xsd:string ;
    dct:description "Personal Data that has undergone a pseudonymisation process or a partial (incomplete) anonymisation process such that it is still considered Personal Data"@en ;
    rdfs:isDefinedBy dpvo: ;
    rdfs:subClassOf dpvo:PersonalData ;
    sw:term_status "accepted"@en .

dpvo:PublicDataSource a owl:NamedIndividual,
        dpvo:DataSource ;
    rdfs:label "Public Data Source"@en ;
    dct:created "2022-01-26"^^xsd:date ;
    dct:creator "Beatriz Esteves"^^xsd:string,
        "Georg P Krog"^^xsd:string,
        "Harshvardhan J. Pandit"^^xsd:string,
        "Julian Flake"^^xsd:string,
        "Paul Ryan"^^xsd:string ;
    dct:description "A source of data that is publicly accessible or available"@en ;
    rdfs:comment "The term 'Public' is used here in a broad sense. Actual consideration of what is 'Public Data' can vary based on several contextual or jurisdictional factors such as  definition of open, methods of access, permissions and licenses."@en ;
    rdfs:isDefinedBy dpvo: ;
    sw:term_status "accepted"@en .

dpvo:PublicInterest a owl:Class ;
    rdfs:label "Public Interest"@en ;
    dct:created "2021-04-21"^^xsd:date ;
    dct:creator "Harshvardhan J. Pandit"^^xsd:string ;
    dct:description "Processing is necessary or beneficial for interest of the public or society at large"@en ;
    rdfs:isDefinedBy dpvo: ;
    rdfs:subClassOf dpvo:LegalBasis ;
    sw:term_status "accepted"@en .

dpvo:PublicLocation a owl:Class ;
    rdfs:label "Public Location"@en ;
    dct:created "2022-10-22"^^xsd:date ;
    dct:creator "Georg P Krog"^^xsd:string ;
    dct:description "Location that is or can be accessed by the public"@en ;
    rdfs:isDefinedBy dpvo: ;
    rdfs:subClassOf dpvo:LocalLocation ;
    sw:term_status "accepted"@en .

dpvo:PublicRelations a owl:Class ;
    rdfs:label "Public Relations"@en ;
    dct:created "2021-09-01"^^xsd:date ;
    dct:creator "David Hickey"^^xsd:string,
        "Georg P Krog"^^xsd:string,
        "Harshvardhan J. Pandit"^^xsd:string,
        "Paul Ryan"^^xsd:string ;
    dct:description "Purposes associated with managing and conducting public relations processes, including creating goodwill for the organisation"@en ;
    dct:source <https://www.privacycommission.be/nl/model-voor-een-register-van-de-verwerkingsactiviteiten> ;
    rdfs:isDefinedBy dpvo: ;
    rdfs:subClassOf dpvo:Marketing ;
    sw:term_status "accepted"@en .

dpvo:QuantumCryptography a owl:Class ;
    rdfs:label "Quantum Cryptography"@en ;
    dct:created "2022-08-17"^^xsd:date ;
    dct:creator "Harshvardhan J. Pandit"^^xsd:string ;
    dct:description "Cryptographic methods that utilise quantum mechanical properties to perform cryptographic tasks"@en ;
    dct:source <https://www.enisa.europa.eu/publications/reference-incident-classification-taxonomy/> ;
    rdfs:isDefinedBy dpvo: ;
    rdfs:subClassOf dpvo:CryptographicMethods ;
    sw:term_status "accepted"@en .

dpvo:Query a owl:Class ;
    rdfs:label "Query"@en ;
    dct:created "2022-06-15"^^xsd:date ;
    dct:creator "Harshvardhan J. Pandit"^^xsd:string ;
    dct:description "to query or make enquiries over data"@en ;
    rdfs:isDefinedBy dpvo: ;
    rdfs:subClassOf dpvo:Consult ;
    sw:term_status "accepted"@en .

dpvo:RNGPseudonymisation a owl:Class ;
    rdfs:label "RNG Pseudonymisation"@en ;
    dct:created "2022-08-17"^^xsd:date ;
    dct:creator "Harshvardhan J. Pandit"^^xsd:string ;
    dct:description "A pseudonymisation method where identifiers are substituted by a number chosen by a Random Number Generator (RNG)"@en ;
    dct:modified "2022-10-13"^^xsd:date ;
    dct:source <https://www.enisa.europa.eu/publications/data-pseudonymisation-advanced-techniques-and-use-cases> ;
    rdfs:isDefinedBy dpvo: ;
    rdfs:subClassOf dpvo:Pseudonymisation ;
    sw:term_status "modified"@en .

dpvo:RandomLocation a owl:NamedIndividual,
        dpvo:LocationFixture ;
    rdfs:label "Random Location"@en ;
    dct:created "2022-06-15"^^xsd:date ;
    dct:creator "Harshvardhan J. Pandit"^^xsd:string ;
    dct:description "Location that is random or unknown"@en ;
    dct:modified "2020-10-05"^^xsd:date ;
    rdfs:isDefinedBy dpvo: ;
    sw:term_status "modified"@en .

dpvo:RecordManagement a owl:Class ;
    rdfs:label "Record Management"@en ;
    dct:created "2021-09-01"^^xsd:date ;
    dct:creator "David Hickey"^^xsd:string,
        "Georg P Krog"^^xsd:string,
        "Harshvardhan J. Pandit"^^xsd:string,
        "Paul Ryan"^^xsd:string ;
    dct:description "Purposes associated with manage creation, storage, and use of records relevant to operations, events, and processes e.g. to store logs or access requests"@en ;
    rdfs:comment "This purpose relates specifiaclly for record creation and management. This can be combined or used along with other purposes to express intentions such as records for legal compliance or vendor payments."@en ;
    rdfs:isDefinedBy dpvo: ;
    rdfs:subClassOf dpvo:Purpose ;
    sw:term_status "accepted"@en .

dpvo:Region a owl:Class ;
    rdfs:label "Region"@en ;
    dct:created "2022-01-19"^^xsd:date ;
    dct:creator "Harshvardhan J. Pandit"^^xsd:string ;
    dct:description "A region is an area or site that is considered a location"@en ;
    rdfs:isDefinedBy dpvo: ;
    rdfs:subClassOf dpvo:Location ;
    sw:term_status "accepted"@en .

dpvo:RegionalAuthority a owl:Class ;
    rdfs:label "Regional Authority"@en ;
    dct:created "2022-02-02"^^xsd:date ;
    dct:creator "Harshvardhan J. Pandit"^^xsd:string ;
    dct:description "An authority tasked with overseeing legal compliance for a region"@en ;
    dct:source <http://purl.org/adms> ;
    rdfs:isDefinedBy dpvo: ;
    rdfs:subClassOf dpvo:Authority ;
    sw:term_status "accepted"@en .

dpvo:RegionalScale a owl:NamedIndividual,
        dpvo:GeographicCoverage ;
    rdfs:label "Regional Scale"@en ;
    dct:created "2022-06-15"^^xsd:date ;
    dct:creator "Harshvardhan J. Pandit"^^xsd:string ;
    dct:description "Geographic coverage spanning a specific region or regions"@en ;
    rdfs:isDefinedBy dpvo: ;
    sw:term_status "accepted"@en .

dpvo:RegisterOfProcessingActivities a owl:Class ;
    rdfs:label "Register of Processing Activities"@en ;
    dct:created "2021-09-08"^^xsd:date ;
    dct:creator "Georg P Krog"^^xsd:string,
        "Harshvardhan J. Pandit"^^xsd:string,
        "Paul Ryan"^^xsd:string ;
    dct:description "A ROPA is a document maintained by Data Controllers detailing processing activities carried out under their responsibility"@en ;
    rdfs:comment "Tied to compliance processes and documents, decide how to specify those"@en ;
    rdfs:isDefinedBy dpvo: ;
    rdfs:subClassOf dpvo:DataProcessingRecord ;
    sw:term_status "accepted"@en .

dpvo:RegularityOfRecertification a owl:Class ;
    rdfs:label "Regularity of Re-certification"@en ;
    dct:created "2019-04-05"^^xsd:date ;
    dct:creator "Axel Polleres"^^xsd:string,
        "Harshvardhan J. Pandit"^^xsd:string,
        "Mark Lizar"^^xsd:string,
        "Rob Brennan"^^xsd:string ;
    dct:description "Policy regarding repetition or renewal of existing certification(s)"@en ;
    rdfs:isDefinedBy dpvo: ;
    rdfs:subClassOf dpvo:OrganisationalMeasure ;
    sw:term_status "accepted"@en .

dpvo:RenewedConsentGiven a owl:NamedIndividual,
        dpvo:ConsentStatusValidForProcessing ;
    rdfs:label "Renewed Consent Given"@en ;
    dct:created "2022-06-22"^^xsd:date ;
    dct:creator "Georg P Krog"^^xsd:string,
        "Harshvardhan J. Pandit"^^xsd:string,
        "Julian Flake"^^xsd:string,
        "Paul Ryan"^^xsd:string ;
    dct:description "The state where a previously given consent has been 'renewed' or 'refreshed' or 'reaffirmed' to form a new instance of given consent"@en ;
    dct:source <https://w3id.org/GConsent> ;
    rdfs:comment "An example of this state is when a previously given consent has expired, and the individual is presented a notice regarding continuing associated processing operations - to which they agree. This state can be useful to keep track of 'reconfirmed' or 'refreshed' consent within consent records, assist notices and contextual agents to create better consenting dialogues, and assist with specific legal obligations related to subsequent consenting"@en ;
    rdfs:isDefinedBy dpvo: ;
    sw:term_status "accepted"@en .

dpvo:RepairImpairments a owl:Class ;
    rdfs:label "Repair Impairments"@en ;
    dct:created "2022-08-24"^^xsd:date ;
    dct:creator "Harshvardhan J. Pandit"^^xsd:string ;
    dct:description "Purposes associated with identifying, rectifying, or otherwise undertaking activities intended to fix or repair impairments to existing functionalities"@en ;
    rdfs:comment "An example of identifying and rectifying impairments is the process of finding and fixing errors in products, commonly referred to as debugging"@en ;
    rdfs:isDefinedBy dpvo: ;
    rdfs:subClassOf dpvo:ServiceProvision ;
    sw:term_status "accepted"@en .

dpvo:RequestAccepted a owl:NamedIndividual,
        dpvo:RequestStatus ;
    rdfs:label "Request Accepted"@en ;
    dct:created "2022-11-30"^^xsd:date ;
    dct:creator "Harshvardhan J. Pandit"^^xsd:string ;
    dct:description "State of a request being accepted towards fulfilment"@en ;
    rdfs:isDefinedBy dpvo: ;
    sw:term_status "accepted"@en .

dpvo:RequestAcknowledged a owl:NamedIndividual,
        dpvo:RequestStatus ;
    rdfs:label "Request Acknowledged"@en ;
    dct:created "2022-11-30"^^xsd:date ;
    dct:creator "Harshvardhan J. Pandit"^^xsd:string ;
    dct:description "State of a request being acknowledged"@en ;
    rdfs:isDefinedBy dpvo: ;
    sw:term_status "accepted"@en .

dpvo:RequestActionDelayed a owl:NamedIndividual,
        dpvo:RequestStatus ;
    rdfs:label "Request Action Delayed"@en ;
    dct:created "2022-11-30"^^xsd:date ;
    dct:creator "Harshvardhan J. Pandit"^^xsd:string ;
    dct:description "State of a request being delayed towards fulfilment"@en ;
    rdfs:isDefinedBy dpvo: ;
    sw:term_status "accepted"@en .

dpvo:RequestFulfilled a owl:NamedIndividual,
        dpvo:RequestStatus ;
    rdfs:label "Request Fulfilled"@en ;
    dct:created "2022-11-30"^^xsd:date ;
    dct:creator "Harshvardhan J. Pandit"^^xsd:string ;
    dct:description "State of a request being fulfilled"@en ;
    rdfs:isDefinedBy dpvo: ;
    sw:term_status "accepted"@en .

dpvo:RequestInitiated a owl:NamedIndividual,
        dpvo:RequestStatus ;
    rdfs:label "Request Initiated"@en ;
    dct:created "2022-11-30"^^xsd:date ;
    dct:creator "Harshvardhan J. Pandit"^^xsd:string ;
    dct:description "State of a request being initiated"@en ;
    rdfs:isDefinedBy dpvo: ;
    sw:term_status "accepted"@en .

dpvo:RequestRejected a owl:NamedIndividual,
        dpvo:RequestStatus ;
    rdfs:label "Request Rejected"@en ;
    dct:created "2022-11-30"^^xsd:date ;
    dct:creator "Harshvardhan J. Pandit"^^xsd:string ;
    dct:description "State of a request being rejected towards non-fulfilment"@en ;
    rdfs:isDefinedBy dpvo: ;
    sw:term_status "accepted"@en .

dpvo:RequestRequiredActionPerformed a owl:NamedIndividual,
        dpvo:RequestStatus ;
    rdfs:label "Request Required Action Performed"@en ;
    dct:created "2022-11-30"^^xsd:date ;
    dct:creator "Harshvardhan J. Pandit"^^xsd:string ;
    dct:description "State of a request's required action having been performed by the other party"@en ;
    rdfs:isDefinedBy dpvo: ;
    sw:term_status "accepted"@en .

dpvo:RequestRequiresAction a owl:NamedIndividual,
        dpvo:RequestStatus ;
    rdfs:label "Request Requires Action"@en ;
    dct:created "2022-11-30"^^xsd:date ;
    dct:creator "Harshvardhan J. Pandit"^^xsd:string ;
    dct:description "State of a request requiring an action to be performed from another party"@en ;
    rdfs:isDefinedBy dpvo: ;
    sw:term_status "accepted"@en .

dpvo:RequestStatusQuery a owl:NamedIndividual,
        dpvo:RequestStatus ;
    rdfs:label "Request Status Query"@en ;
    dct:created "2022-11-30"^^xsd:date ;
    dct:creator "Harshvardhan J. Pandit"^^xsd:string ;
    dct:description "State of a request's status being queried"@en ;
    rdfs:isDefinedBy dpvo: ;
    sw:term_status "accepted"@en .

dpvo:RequestUnfulfilled a owl:NamedIndividual,
        dpvo:RequestStatus ;
    rdfs:label "Request Unfulfilled"@en ;
    dct:created "2022-11-30"^^xsd:date ;
    dct:creator "Harshvardhan J. Pandit"^^xsd:string ;
    dct:description "State of a request being unfulfilled"@en ;
    rdfs:isDefinedBy dpvo: ;
    sw:term_status "accepted"@en .

dpvo:Required a owl:NamedIndividual,
        dpvo:Necessity ;
    rdfs:label "Required"@en ;
    dct:created "2022-02-13"^^xsd:date ;
    dct:creator "Beatriz Esteves"^^xsd:string,
        "Georg P Krog"^^xsd:string,
        "Harshvardhan J. Pandit"^^xsd:string,
        "Julian Flake"^^xsd:string,
        "Paul Ryan"^^xsd:string ;
    dct:description "Indication of 'required' or 'necessary'"@en ;
    rdfs:isDefinedBy dpvo: ;
    sw:term_status "accepted"@en .

dpvo:Restrict a owl:Class ;
    rdfs:label "Restrict"@en ;
    dct:created "2019-05-07"^^xsd:date ;
    dct:description "to apply a restriction on the processsing of specific records"@en ;
    dct:source <https://eur-lex.europa.eu/eli/reg/2016/679/art_4/par_2/oj> ;
    rdfs:isDefinedBy dpvo: ;
    rdfs:subClassOf dpvo:Transform ;
    sw:term_status "accepted"@en .

dpvo:Retrieve a owl:Class ;
    rdfs:label "Retrieve"@en ;
    dct:created "2019-05-07"^^xsd:date ;
    dct:description "to retrieve data, often in an automated manner"@en ;
    dct:source <https://eur-lex.europa.eu/eli/reg/2016/679/art_4/par_2/oj> ;
    rdfs:isDefinedBy dpvo: ;
    rdfs:subClassOf dpvo:Use ;
    sw:term_status "accepted"@en .

dpvo:ReviewImpactAssessment a owl:Class ;
    rdfs:label "Review Impact Assessment"@en ;
    dct:created "2022-10-22"^^xsd:date ;
    dct:creator "Georg P Krog"^^xsd:string,
        "Harshvardhan J. Pandit"^^xsd:string ;
    dct:description "Procedures to review impact assessments in terms of continued validity, adequacy for intended purposes, and conformance of processes with findings"@en ;
    rdfs:isDefinedBy dpvo: ;
    rdfs:subClassOf dpvo:ImpactAssessment,
        dpvo:ReviewProcedure ;
    sw:term_status "accepted"@en .

dpvo:RightExerciseActivity a owl:Class ;
    rdfs:label "Right Exercise Activity"@en ;
    dct:created "2022-11-02"^^xsd:date ;
    dct:creator "Beatriz Esteves"^^xsd:string,
        "Georg P Krog"^^xsd:string,
        "Harshvardhan J Pandit"^^xsd:string,
        "Paul Ryan"^^xsd:string ;
    dct:description "An activity representing an exercising of an active right"@en ;
    rdfs:comment "There may be multiple activities associated with exercising and fulfilling rights. See the RightExerciseRecord concept for record-keeping of such activities in a cohesive manner."@en ;
    rdfs:isDefinedBy dpvo: ;
    sw:term_status "accepted"@en .

dpvo:RightExerciseRecord a owl:NamedIndividual,
        dpvo:Record ;
    rdfs:label "Right Exercise Record"@en ;
    dct:created "2022-11-02"^^xsd:date ;
    dct:creator "Beatriz Esteves"^^xsd:string,
        "Georg P Krog"^^xsd:string,
        "Harshvardhan J Pandit"^^xsd:string,
        "Paul Ryan"^^xsd:string ;
    dct:description "Record of a Right being exercised"@en ;
    rdfs:comment "This concept represents a record of one or more right exercise activities, such as those associated with a single data subject or service or entity"@en ;
    rdfs:isDefinedBy dpvo: ;
    sw:term_status "accepted"@en .

dpvo:RightFulfilmentNotice a owl:Class ;
    rdfs:label "Right Fulfilment Notice"@en ;
    dct:created "2022-11-02"^^xsd:date ;
    dct:creator "Beatriz Esteves"^^xsd:string,
        "Harshvardhan J. Pandit"^^xsd:string ;
    dct:description "Notice provided regarding fulfilment of a right"@en ;
    rdfs:comment "This notice is associated with situations where information is provided with the intention of progressing the fulfilment of a right. For example, a notice asking for more information regarding the scope of the right, or providing information on where to access the data provided under a right."@en ;
    rdfs:isDefinedBy dpvo: ;
    rdfs:subClassOf dpvo:Notice ;
    sw:term_status "accepted"@en .

dpvo:RightNonFulfilmentNotice a owl:Class ;
    rdfs:label "Right Non-Fulfilment Notice"@en ;
    dct:created "2022-11-02"^^xsd:date ;
    dct:creator "Beatriz Esteves"^^xsd:string,
        "Harshvardhan J. Pandit"^^xsd:string ;
    dct:description "Notice provided regarding non-fulfilment of a right"@en ;
    rdfs:comment "This notice is associated with situations where information is provided with the intention of communicating non-fulfilment of a right. For example, to provide justifications on why a right could not be fulfilled or providing information about another entity  who should be approached for exercising this right."@en ;
    rdfs:isDefinedBy dpvo: ;
    rdfs:subClassOf dpvo:Notice ;
    sw:term_status "accepted"@en .

dpvo:RiskManagementPlan a owl:Class ;
    rdfs:label "Risk Management Plan"@en ;
    dct:created "2022-08-18"^^xsd:date ;
    dct:creator "Harshvardhan J. Pandit"^^xsd:string ;
    dct:description "A scheme within the risk management framework specifying the approach, the management components, and resources to be applied to the management of risk"@en ;
    dct:source <https://www.iso.org/standard/79637.html> ;
    rdfs:isDefinedBy dpvo: ;
    rdfs:subClassOf dpvo:SecurityProcedure ;
    sw:term_status "accepted"@en .

dpvo:RiskManagementPolicy a owl:Class ;
    rdfs:label "Risk Management Policy"@en ;
    dct:created "2022-08-18"^^xsd:date ;
    dct:creator "Harshvardhan J. Pandit"^^xsd:string ;
    dct:description "A policy or statement of the overall intentions and direction of an organisation related to risk management"@en ;
    dct:source <https://www.iso.org/standard/79637.html> ;
    rdfs:isDefinedBy dpvo: ;
    rdfs:subClassOf dpvo:Policy,
        dpvo:SecurityProcedure ;
    sw:term_status "accepted"@en .

dpvo:RiskManagementProcess a owl:Class ;
    rdfs:label "Risk Management Process"@en ;
    dct:created "2022-08-18"^^xsd:date ;
    dct:creator "Harshvardhan J. Pandit"^^xsd:string ;
    dct:description "The systematic application of management policies, procedures and practices to the activities of communicating, consulting, establishing the context, and identifying, analysing, evaluating, treating, monitoring, and reviewing risk"@en ;
    dct:source <https://www.iso.org/iso-31000-risk-management.html>,
        <https://www.iso.org/standard/79637.html> ;
    rdfs:isDefinedBy dpvo: ;
    rdfs:subClassOf dpvo:SecurityProcedure ;
    sw:term_status "accepted"@en .

dpvo:SafeguardForDataTransfer a owl:Class ;
    rdfs:label "Safeguard for Data Transfer"@en ;
    dct:created "2021-09-22"^^xsd:date ;
    dct:creator "David Hickey"^^xsd:string,
        "Georg P Krog"^^xsd:string,
        "Harshvardhan J. Pandit"^^xsd:string,
        "Paul Ryan"^^xsd:string ;
    dct:description "Represents a safeguard used for data transfer. Can include technical or organisational measures."@en ;
    rdfs:isDefinedBy dpvo: ;
    rdfs:subClassOf dpvo:Safeguard ;
    sw:term_status "accepted"@en .

dpvo:ScoringOfIndividuals a owl:Class ;
    rdfs:label "Scoring of Individuals"@en ;
    dct:created "2022-10-22"^^xsd:date ;
    dct:creator "Harshvardhan J. Pandit"^^xsd:string ;
    dct:description "Processing that involves scoring of individuals"@en ;
    dct:modified "2022-11-30"^^xsd:date ;
    dct:source <https://eur-lex.europa.eu/eli/reg/2016/679/art_4/par_2/oj> ;
    rdfs:isDefinedBy dpvo: ;
    rdfs:subClassOf dpvo:EvaluationScoring ;
    sw:term_status "modified"@en .

dpvo:Screen a owl:Class ;
    rdfs:label "Screen"@en ;
    dct:created "2022-06-15"^^xsd:date ;
    dct:creator "Georg P Krog"^^xsd:string,
        "Harshvardhan J. Pandit"^^xsd:string ;
    dct:description "to remove data for some criteria"@en ;
    rdfs:isDefinedBy dpvo: ;
    rdfs:subClassOf dpvo:Transform ;
    sw:term_status "accepted"@en .

dpvo:Seal a owl:Class ;
    rdfs:label "Seal"@en ;
    dct:created "2019-04-05"^^xsd:date ;
    dct:creator "Axel Polleres"^^xsd:string,
        "Harshvardhan J. Pandit"^^xsd:string,
        "Mark Lizar"^^xsd:string,
        "Rob Brennan"^^xsd:string ;
    dct:description "A seal or a mark indicating proof of certification to some certification or standard"@en ;
    rdfs:isDefinedBy dpvo: ;
    rdfs:subClassOf dpvo:CertificationSeal ;
    sw:term_status "accepted"@en .

dpvo:SearchFunctionalities a owl:Class ;
    rdfs:label "Search Functionalities"@en ;
    dct:created "2022-11-09"^^xsd:date ;
    dct:creator "Georg P Krog"^^xsd:string ;
    dct:description "Purposes associated with providing searching, querying, or other forms of information retrieval related functionalities"@en ;
    rdfs:isDefinedBy dpvo: ;
    rdfs:subClassOf dpvo:ServiceProvision ;
    sw:term_status "accepted"@en .

dpvo:SecondaryImportance a owl:NamedIndividual,
        dpvo:Importance ;
    rdfs:label "Secondary Importance"@en ;
    dct:created "2022-02-11"^^xsd:date ;
    dct:creator "Beatriz Esteves"^^xsd:string,
        "Georg P Krog"^^xsd:string,
        "Harshvardhan J. Pandit"^^xsd:string,
        "Julian Flake"^^xsd:string,
        "Paul Ryan"^^xsd:string ;
    dct:description "Indication of 'secondary' or 'minor' or 'auxiliary' importance"@en ;
    rdfs:isDefinedBy dpvo: ;
    sw:term_status "accepted"@en .

dpvo:SecretSharingSchemes a owl:Class ;
    rdfs:label "Secret Sharing Schemes"@en ;
    dct:created "2022-08-17"^^xsd:date ;
    dct:creator "Harshvardhan J. Pandit"^^xsd:string ;
    dct:description "Use of secret sharing schemes where the secret can only be reconstructed through combination of sufficient number of individuals"@en ;
    dct:source <https://www.enisa.europa.eu/publications/data-pseudonymisation-advanced-techniques-and-use-cases> ;
    rdfs:isDefinedBy dpvo: ;
    rdfs:subClassOf dpvo:CryptographicMethods ;
    sw:term_status "accepted"@en .

dpvo:SecureMultiPartyComputation a owl:Class ;
    rdfs:label "Secure Multi-Party Computation"@en ;
    dct:created "2022-08-17"^^xsd:date ;
    dct:creator "Harshvardhan J. Pandit"^^xsd:string ;
    dct:description "Use of cryptographic methods for entities to jointly compute functions without revealing inputs"@en ;
    dct:source <https://www.enisa.europa.eu/publications/reference-incident-classification-taxonomy/> ;
    rdfs:isDefinedBy dpvo: ;
    rdfs:subClassOf dpvo:CryptographicMethods ;
    sw:term_status "accepted"@en .

dpvo:SecurityKnowledgeTraining a owl:Class ;
    rdfs:label "Security Knowledge Training"@en ;
    dct:created "2022-08-17"^^xsd:date ;
    dct:creator "Harshvardhan J. Pandit"^^xsd:string ;
    dct:description "Training intended to increase knowledge regarding security"@en ;
    dct:source <https://www.enisa.europa.eu/publications/5g-cybersecurity-standards> ;
    rdfs:isDefinedBy dpvo: ;
    rdfs:subClassOf dpvo:StaffTraining ;
    sw:term_status "accepted"@en .

dpvo:SecurityRoleProcedures a owl:Class ;
    rdfs:label "Security Role Procedures"@en ;
    dct:created "2022-08-17"^^xsd:date ;
    dct:creator "Harshvardhan J. Pandit"^^xsd:string ;
    dct:description "Procedures related to security roles"@en ;
    dct:source <https://www.enisa.europa.eu/publications/5g-cybersecurity-standards> ;
    rdfs:isDefinedBy dpvo: ;
    rdfs:subClassOf dpvo:SecurityProcedure ;
    sw:term_status "accepted"@en .

dpvo:SellDataToThirdParties a owl:Class ;
    rdfs:label "Sell Data to Third Parties"@en ;
    dct:created "2019-04-05"^^xsd:date ;
    dct:creator "Axel Polleres"^^xsd:string,
        "Elmar Kiesling"^^xsd:string,
        "Fajar Ekaputra"^^xsd:string,
        "Harshvardhan J. Pandit"^^xsd:string,
        "Javier Fernandez"^^xsd:string,
        "Simon Steyskal"^^xsd:string ;
    dct:description "Purposes associated with selling or sharing data or information to third parties"@en ;
    rdfs:comment "Sell here means exchange, submit, or provide in return for direct or indirect compensation. Was subclass of commercial interest, changed to reflect selling something"@en ;
    rdfs:isDefinedBy dpvo: ;
    rdfs:subClassOf dpvo:SellProducts ;
    sw:term_status "accepted"@en .

dpvo:SellInsightsFromData a owl:Class ;
    rdfs:label "Sell Insights from Data"@en ;
    dct:created "2019-04-05"^^xsd:date ;
    dct:creator "Axel Polleres"^^xsd:string,
        "Elmar Kiesling"^^xsd:string,
        "Fajar Ekaputra"^^xsd:string,
        "Harshvardhan J. Pandit"^^xsd:string,
        "Javier Fernandez"^^xsd:string,
        "Simon Steyskal"^^xsd:string ;
    dct:description "Purposes associated with selling or sharing insights obtained from analysis of data"@en ;
    rdfs:comment "Sell here means exchange, submit, or provide in return for direct or indirect compensation. Was subclass of commercial interest, changed to reflect selling something"@en ;
    rdfs:isDefinedBy dpvo: ;
    rdfs:subClassOf dpvo:SellProducts ;
    sw:term_status "accepted"@en .

dpvo:SellProductsToDataSubject a owl:Class ;
    rdfs:label "Sell Products to Data Subject"@en ;
    dct:created "2019-04-05"^^xsd:date ;
    dct:creator "Axel Polleres"^^xsd:string,
        "Elmar Kiesling"^^xsd:string,
        "Fajar Ekaputra"^^xsd:string,
        "Harshvardhan J. Pandit"^^xsd:string,
        "Javier Fernandez"^^xsd:string,
        "Simon Steyskal"^^xsd:string ;
    dct:description "Purposes associated with selling products or services to the user, consumer, or data subjects"@en ;
    rdfs:comment "Sell Products here refers to processing necessary to provide and complete a sale to customers. It should not be confused with providing services with a cost based on an established agreement."@en ;
    rdfs:isDefinedBy dpvo: ;
    rdfs:subClassOf dpvo:SellProducts ;
    sw:term_status "accepted"@en .

dpvo:ServiceRegistration a owl:Class ;
    rdfs:label "Service Registration"@en ;
    dct:created "2020-11-04"^^xsd:date ;
    dct:creator "Beatriz Esteves"^^xsd:string,
        "Georg P Krog"^^xsd:string,
        "Harshvardhan J. Pandit"^^xsd:string ;
    dct:description "Purposes associated with registering users and collecting information required for providing a service"@en ;
    rdfs:comment "An example of service registration is to provide a form that collects information such as preferred language or media format for downloading a movie"@en ;
    rdfs:isDefinedBy dpvo: ;
    rdfs:subClassOf dpvo:ServiceProvision ;
    sw:term_status "accepted"@en .

dpvo:ServiceUsageAnalytics a owl:Class ;
    rdfs:label "Service Usage Analytics"@en ;
    dct:created "2020-11-04"^^xsd:date ;
    dct:creator "Beatriz Esteves"^^xsd:string,
        "Georg P Krog"^^xsd:string,
        "Harshvardhan J. Pandit"^^xsd:string ;
    dct:description "Purposes associated with conducting analysis and reporting related to usage of services or products"@en ;
    dct:modified "2022-10-05"^^xsd:date ;
    rdfs:comment "Was \"UsageAnalytics\", prefixed with Service to better reflect scope"@en ;
    rdfs:isDefinedBy dpvo: ;
    rdfs:subClassOf dpvo:ServiceProvision ;
    sw:term_status "modified"@en .

dpvo:Share a owl:Class ;
    rdfs:label "Share"@en ;
    dct:created "2019-05-07"^^xsd:date ;
    dct:description "to give data (or a portion of it) to others"@en ;
    dct:source <https://eur-lex.europa.eu/eli/reg/2016/679/art_4/par_2/oj> ;
    rdfs:isDefinedBy dpvo: ;
    rdfs:subClassOf dpvo:Disclose ;
    sw:term_status "accepted"@en .

dpvo:SingleSignOn a owl:Class ;
    rdfs:label "Single Sign On"@en ;
    dct:created "2020-11-04"^^xsd:date ;
    dct:creator "Georg P Krog"^^xsd:string,
        "Harshvardhan J. Pandit"^^xsd:string,
        "Paul Ryan"^^xsd:string ;
    dct:description "Use of credentials or processes that enable using one set of credentials to authenticate multiple contexts."@en ;
    rdfs:isDefinedBy dpvo: ;
    rdfs:subClassOf dpvo:AuthenticationProtocols ;
    sw:term_status "accepted"@en .

dpvo:SingularDataVolume a owl:NamedIndividual,
        dpvo:DataVolume ;
    rdfs:label "Singular Data Volume"@en ;
    dct:created "2022-06-15"^^xsd:date ;
    dct:creator "Harshvardhan J. Pandit"^^xsd:string ;
    dct:description "Data volume that is considered singular i.e. a specific instance or single item"@en ;
    rdfs:isDefinedBy dpvo: ;
    sw:term_status "accepted"@en .

dpvo:SingularFrequency a owl:Class ;
    rdfs:label "Singular Frequency"@en ;
    dct:created "2022-06-15"^^xsd:date ;
    dct:creator "Harshvardhan J. Pandit"^^xsd:string ;
    dct:description "Frequency where occurences are singular i.e. they take place only once"@en ;
    dct:modified "2020-10-05"^^xsd:date ;
    rdfs:isDefinedBy dpvo: ;
    rdfs:subClassOf dpvo:Frequency ;
    sw:term_status "modified"@en .

dpvo:SingularScaleOfDataSubjects a owl:NamedIndividual,
        dpvo:DataSubjectScale ;
    rdfs:label "Singular Scale Of Data Subjects"@en ;
    dct:created "2022-06-15"^^xsd:date ;
    dct:creator "Harshvardhan J. Pandit"^^xsd:string ;
    dct:description "Scale of data subjects considered singular i.e. a specific data subject"@en ;
    rdfs:isDefinedBy dpvo: ;
    sw:term_status "accepted"@en .

dpvo:SmallDataVolume a owl:NamedIndividual,
        dpvo:DataVolume ;
    rdfs:label "Small Data Volume"@en ;
    dct:created "2022-06-15"^^xsd:date ;
    dct:creator "Harshvardhan J. Pandit"^^xsd:string ;
    dct:description "Data volume that is considered small or limited within the context"@en ;
    rdfs:isDefinedBy dpvo: ;
    sw:term_status "accepted"@en .

dpvo:SmallScaleOfDataSubjects a owl:NamedIndividual,
        dpvo:DataSubjectScale ;
    rdfs:label "Small Scale Of Data Subjects"@en ;
    dct:created "2022-06-15"^^xsd:date ;
    dct:creator "Harshvardhan J. Pandit"^^xsd:string ;
    dct:description "Scale of data subjects considered small or limited within the context"@en ;
    rdfs:isDefinedBy dpvo: ;
    sw:term_status "accepted"@en .

dpvo:SmallScaleProcessing a owl:NamedIndividual,
        dpvo:ProcessingScale ;
    rdfs:label "Small Scale Processing"@en ;
    dct:created "2022-09-07"^^xsd:date ;
    dct:creator "Harshvardhan J. Pandit"^^xsd:string ;
    dct:description "Processing that takes place at small scales (as specified by some criteria)"@en ;
    rdfs:isDefinedBy dpvo: ;
    sw:term_status "accepted"@en .

dpvo:SocialMediaMarketing a owl:Class ;
    rdfs:label "Social Media Marketing"@en ;
    dct:created "2020-11-04"^^xsd:date ;
    dct:creator "Beatriz Esteves"^^xsd:string,
        "Georg P Krog"^^xsd:string,
        "Harshvardhan J. Pandit"^^xsd:string ;
    dct:description "Purposes associated with conducting marketing through social media"@en ;
    rdfs:isDefinedBy dpvo: ;
    rdfs:subClassOf dpvo:Marketing ;
    sw:term_status "accepted"@en .

dpvo:SpecialCategoryPersonalData a owl:Class ;
    rdfs:label "Special Category Personal Data"@en ;
    dct:created "2019-05-07"^^xsd:date ;
    dct:creator "Elmar Kiesling; Harshvardhan J. Pandit"^^xsd:string,
        "Fajar Ekaputra"^^xsd:string ;
    dct:description "Sensitive Personal Data whose use requires specific legal permission or justification"@en ;
    dct:modified "2022-01-19"^^xsd:date ;
    dct:source <https://eur-lex.europa.eu/eli/reg/2016/679/art_9/par_1/oj> ;
    rdfs:comment "The term 'special category' is based on GDPR Art.9, but should not be considered as exlusive to it. DPV considers all Special Categories to also be Sensitive, but whose use is either prohibited or regulated and therefore requires additional legal basis for justification."@en ;
    rdfs:isDefinedBy dpvo: ;
    rdfs:subClassOf dpvo:SensitivePersonalData ;
    sw:term_status "modified"@en .

dpvo:SporadicDataVolume a owl:NamedIndividual,
        dpvo:DataVolume ;
    rdfs:label "Sporadic Data Volume"@en ;
    dct:created "2022-06-15"^^xsd:date ;
    dct:creator "Harshvardhan J. Pandit"^^xsd:string ;
    dct:description "Data volume that is considered sporadic or sparse within the context"@en ;
    rdfs:isDefinedBy dpvo: ;
    sw:term_status "accepted"@en .

dpvo:SporadicFrequency a owl:Class ;
    rdfs:label "Sporadic Frequency"@en ;
    dct:created "2022-06-15"^^xsd:date ;
    dct:creator "Harshvardhan J. Pandit"^^xsd:string ;
    dct:description "Frequency where occurences are sporadic or infrequent or sparse"@en ;
    dct:modified "2020-10-05"^^xsd:date ;
    rdfs:isDefinedBy dpvo: ;
    rdfs:subClassOf dpvo:Frequency ;
    sw:term_status "modified"@en .

dpvo:SporadicScaleOfDataSubjects a owl:NamedIndividual,
        dpvo:DataSubjectScale ;
    rdfs:label "Sporadic Scale Of Data Subjects"@en ;
    dct:created "2022-06-15"^^xsd:date ;
    dct:creator "Harshvardhan J. Pandit"^^xsd:string ;
    dct:description "Scale of data subjects considered sporadic or sparse within the context"@en ;
    rdfs:isDefinedBy dpvo: ;
    sw:term_status "accepted"@en .

dpvo:StorageDeletion a owl:Class ;
    rdfs:label "Storage Deletion"@en ;
    dct:created "2019-04-05"^^xsd:date ;
    dct:creator "Axel Polleres"^^xsd:string,
        "Harshvardhan J. Pandit"^^xsd:string,
        "Mark Lizar"^^xsd:string,
        "Rob Brennan"^^xsd:string ;
    dct:description "Deletion or Erasure of data including any deletion guarantees"@en ;
    rdfs:isDefinedBy dpvo: ;
    rdfs:subClassOf dpvo:StorageCondition ;
    sw:term_status "accepted"@en .

dpvo:StorageDuration a owl:Class ;
    rdfs:label "Storage Duration"@en ;
    dct:created "2019-04-05"^^xsd:date ;
    dct:creator "Axel Polleres"^^xsd:string,
        "Harshvardhan J. Pandit"^^xsd:string,
        "Mark Lizar"^^xsd:string,
        "Rob Brennan"^^xsd:string ;
    dct:description "Duration or temporal limitation on storage of personal data"@en ;
    rdfs:isDefinedBy dpvo: ;
    rdfs:subClassOf dpvo:Duration,
        dpvo:StorageCondition ;
    sw:term_status "accepted"@en .

dpvo:StorageLocation a owl:Class ;
    rdfs:label "Storage Location"@en ;
    dct:created "2019-04-05"^^xsd:date ;
    dct:creator "Axel Polleres"^^xsd:string,
        "Harshvardhan J. Pandit"^^xsd:string,
        "Mark Lizar"^^xsd:string,
        "Rob Brennan"^^xsd:string ;
    dct:description "Location or geospatial scope where the data is stored"@en ;
    rdfs:isDefinedBy dpvo: ;
    rdfs:subClassOf dpvo:Location,
        dpvo:StorageCondition ;
    sw:term_status "accepted"@en .

dpvo:StorageRestoration a owl:Class ;
    rdfs:label "Storage Restoration"@en ;
    dct:created "2019-04-05"^^xsd:date ;
    dct:creator "Axel Polleres"^^xsd:string,
        "Harshvardhan J. Pandit"^^xsd:string,
        "Mark Lizar"^^xsd:string,
        "Rob Brennan"^^xsd:string ;
    dct:description "Regularity and temporal span of data restoration/backup mechanisms that guarantee that data is preserved"@en ;
    rdfs:isDefinedBy dpvo: ;
    rdfs:subClassOf dpvo:StorageCondition ;
    sw:term_status "accepted"@en .

dpvo:Store a owl:Class ;
    rdfs:label "Store"@en ;
    dct:created "2019-05-07"^^xsd:date ;
    dct:description "to keep data for future use"@en ;
    dct:source <https://eur-lex.europa.eu/eli/reg/2016/679/art_4/par_2/oj> ;
    rdfs:isDefinedBy dpvo: ;
    rdfs:subClassOf dpvo:Processing ;
    sw:term_status "accepted"@en .

dpvo:Structure a owl:Class ;
    rdfs:label "Structure"@en ;
    dct:created "2019-05-07"^^xsd:date ;
    dct:description "to arrange data according to a structure"@en ;
    dct:source <https://eur-lex.europa.eu/eli/reg/2016/679/art_4/par_2/oj> ;
    rdfs:isDefinedBy dpvo: ;
    rdfs:subClassOf dpvo:Organise ;
    sw:term_status "accepted"@en .

dpvo:Student a owl:Class ;
    rdfs:label "Student"@en ;
    dct:created "2022-04-06"^^xsd:date ;
    dct:creator "Beatriz Esteves"^^xsd:string,
        "Georg P. Krog"^^xsd:string,
        "Harshvardhan J. Pandit"^^xsd:string,
        "Julian Flake"^^xsd:string,
        "Paul Ryan"^^xsd:string ;
    dct:description "Data subjects that are students"@en ;
    rdfs:isDefinedBy dpvo: ;
    rdfs:subClassOf dpvo:DataSubject ;
    sw:term_status "accepted"@en .

dpvo:SubProcessorAgreement a owl:Class ;
    rdfs:label "Sub-Processor Agreement"@en ;
    dct:created "2022-01-26"^^xsd:date ;
    dct:creator "Beatriz Esteves"^^xsd:string,
        "Georg P Krog"^^xsd:string,
        "Harshvardhan J. Pandit"^^xsd:string,
        "Julian Flake"^^xsd:string,
        "Paul Ryan"^^xsd:string ;
    dct:description "An agreement outlining conditions, criteria, obligations, responsibilities, and specifics for carrying out processing of personal data between a Data Processor and a Data (Sub-)Processor"@en ;
    rdfs:isDefinedBy dpvo: ;
    rdfs:subClassOf dpvo:DataProcessingAgreement ;
    sw:term_status "accepted"@en .

dpvo:Subscriber a owl:Class ;
    rdfs:label "Subscriber"@en ;
    dct:created "2022-04-06"^^xsd:date ;
    dct:creator "Beatriz Esteves"^^xsd:string,
        "Georg P. Krog"^^xsd:string,
        "Harshvardhan J. Pandit"^^xsd:string,
        "Julian Flake"^^xsd:string,
        "Paul Ryan"^^xsd:string ;
    dct:description "Data subjects that subscribe to service(s)"@en ;
    rdfs:comment "note: subscriber can be customer or consumer"@en ;
    rdfs:isDefinedBy dpvo: ;
    rdfs:subClassOf dpvo:DataSubject ;
    sw:term_status "accepted"@en .

dpvo:SupraNationalAuthority a owl:Class ;
    rdfs:label "Supra-National Authority"@en ;
    dct:created "2022-02-02"^^xsd:date ;
    dct:creator "Harshvardhan J. Pandit"^^xsd:string ;
    dct:description "An authority tasked with overseeing legal compliance for a supra-national union e.g. EU"@en ;
    dct:source <http://purl.org/adms> ;
    rdfs:isDefinedBy dpvo: ;
    rdfs:subClassOf dpvo:Authority ;
    sw:term_status "accepted"@en .

dpvo:SupraNationalUnion a owl:Class ;
    rdfs:label "Supranational Union"@en ;
    dct:created "2022-01-19"^^xsd:date ;
    dct:creator "Harshvardhan J. Pandit"^^xsd:string ;
    dct:description "A political union of two or more countries with an establishment of common authority"@en ;
    rdfs:isDefinedBy dpvo: ;
    rdfs:subClassOf dpvo:Location ;
    sw:term_status "accepted"@en .

dpvo:SymmetricCryptography a owl:Class ;
    rdfs:label "Symmetric Cryptography"@en ;
    dct:created "2022-08-17"^^xsd:date ;
    dct:creator "Harshvardhan J. Pandit"^^xsd:string ;
    dct:description "Use of cryptography where the same keys are utilised for encryption and descryption of information"@en ;
    dct:source <https://www.enisa.europa.eu/publications/reference-incident-classification-taxonomy/> ;
    rdfs:isDefinedBy dpvo: ;
    rdfs:subClassOf dpvo:CryptographicMethods ;
    sw:term_status "accepted"@en .

dpvo:SymmetricEncryption a owl:Class ;
    rdfs:label "Symmetric Encryption"@en ;
    dct:created "2022-08-17"^^xsd:date ;
    dct:creator "Harshvardhan J. Pandit"^^xsd:string ;
    dct:description "Use of symmetric cryptography to encrypt data"@en ;
    dct:source <https://www.enisa.europa.eu/publications/data-pseudonymisation-advanced-techniques-and-use-cases> ;
    rdfs:isDefinedBy dpvo: ;
    rdfs:subClassOf dpvo:Encryption ;
    sw:term_status "accepted"@en .

dpvo:SyntheticData a owl:Class ;
    rdfs:label "Synthetic Data"@en ;
    dct:created "2022-08-18"^^xsd:date ;
    dct:creator "Harshvardhan J. Pandit"^^xsd:string ;
    dct:description "Synthetic data reffers to artificially created data such that it is intended to resemble real data (personal or non-personal), but does not refer to any specific identified or identifiable individual, or to the real measure of an observable parameter in the case of non-personal data"@en ;
    dct:source <https://www.enisa.europa.eu/publications/data-protection-engineering> ;
    rdfs:isDefinedBy dpvo: ;
    rdfs:subClassOf dpvo:Data ;
    sw:term_status "accepted"@en .

dpvo:SystematicMonitoring a owl:Class ;
    rdfs:label "Systematic Monitoring"@en ;
    dct:created "2020-11-04"^^xsd:date ;
    dct:creator "Harshvardhan J. Pandit"^^xsd:string,
        "Piero Bonatti"^^xsd:string ;
    dct:description "Processing that involves systematic monitoring of individuals"@en ;
    dct:source <https://eur-lex.europa.eu/eli/reg/2016/679/art_4/par_2/oj> ;
    rdfs:isDefinedBy dpvo: ;
    rdfs:subClassOf dpvo:ProcessingContext ;
    sw:term_status "accepted"@en .

dpvo:TargetedAdvertising a owl:Class ;
    rdfs:label "Targeted Advertising"@en ;
    dct:created "2022-03-30"^^xsd:date ;
    dct:creator "Harshvardhan J. Pandit"^^xsd:string ;
    dct:description "Purposes associated with creating and providing pesonalised advertisement where the personalisation is targeted to a specific individual or group of individuals"@en ;
    rdfs:isDefinedBy dpvo: ;
    rdfs:subClassOf dpvo:PersonalisedAdvertising ;
    sw:term_status "accepted"@en .

dpvo:TechnicalServiceProvision a owl:Class ;
    rdfs:label "Technical Service Provision"@en ;
    dct:created "2021-09-08"^^xsd:date ;
    dct:creator "Harshvardhan J. Pandit"^^xsd:string ;
    dct:description "Purposes associated with managing and providing technical processes and functions necessary for delivering services"@en ;
    rdfs:isDefinedBy dpvo: ;
    rdfs:subClassOf dpvo:ServiceProvision ;
    sw:term_status "accepted"@en .

dpvo:TemporalDuration a owl:Class ;
    rdfs:label "Temporal Duration"@en ;
    dct:created "2022-06-15"^^xsd:date ;
    dct:creator "Harshvardhan J. Pandit"^^xsd:string ;
    dct:description "Duration that has a fixed temporal duration e.g. 6 months"@en ;
    dct:modified "2020-10-05"^^xsd:date ;
    rdfs:isDefinedBy dpvo: ;
    rdfs:subClassOf dpvo:Duration ;
    sw:term_status "modified"@en .

dpvo:ThirdPartyAgreement a owl:Class ;
    rdfs:label "Third-Party Agreement"@en ;
    dct:created "2022-02-09"^^xsd:date ;
    dct:creator "Harshvardhan J. Pandit"^^xsd:string ;
    dct:description "An agreement outlining conditions, criteria, obligations, responsibilities, and specifics for carrying out processing of personal data between a Data Controller or Processor and a Third Party"@en ;
    rdfs:isDefinedBy dpvo: ;
    rdfs:subClassOf dpvo:DataProcessingAgreement ;
    sw:term_status "accepted"@en .

dpvo:ThirdPartySecurityProcedures a owl:Class ;
    rdfs:label "Third Party Security Procedures"@en ;
    dct:created "2022-08-17"^^xsd:date ;
    dct:creator "Harshvardhan J. Pandit"^^xsd:string ;
    dct:description "Procedures related to security associated with Third Parties"@en ;
    dct:source <https://www.enisa.europa.eu/publications/5g-cybersecurity-standards> ;
    rdfs:isDefinedBy dpvo: ;
    rdfs:subClassOf dpvo:SecurityProcedure ;
    sw:term_status "accepted"@en .

dpvo:Tourist a owl:Class ;
    rdfs:label "Tourist"@en ;
    dct:created "2022-04-06"^^xsd:date ;
    dct:creator "Beatriz Esteves"^^xsd:string,
        "Georg P. Krog"^^xsd:string,
        "Harshvardhan J. Pandit"^^xsd:string,
        "Julian Flake"^^xsd:string,
        "Paul Ryan"^^xsd:string ;
    dct:description "Data subjects that are tourists i.e. not citizens and not immigrants"@en ;
    rdfs:isDefinedBy dpvo: ;
    rdfs:subClassOf dpvo:DataSubject ;
    sw:term_status "accepted"@en .

dpvo:Transmit a owl:Class ;
    rdfs:label "Transmit"@en ;
    dct:created "2019-05-07"^^xsd:date ;
    dct:description "to send out data"@en ;
    dct:source <https://eur-lex.europa.eu/eli/reg/2016/679/art_4/par_2/oj> ;
    rdfs:isDefinedBy dpvo: ;
    rdfs:subClassOf dpvo:Disclose ;
    sw:term_status "accepted"@en .

dpvo:TrustedComputing a owl:Class ;
    rdfs:label "Trusted Computing"@en ;
    dct:created "2022-08-17"^^xsd:date ;
    dct:creator "Harshvardhan J. Pandit"^^xsd:string ;
    dct:description "Use of cryptographic methods to restrict access and execution to trusted parties and code"@en ;
    dct:source <https://www.enisa.europa.eu/publications/reference-incident-classification-taxonomy/> ;
    rdfs:isDefinedBy dpvo: ;
    rdfs:subClassOf dpvo:CryptographicMethods ;
    sw:term_status "accepted"@en .

dpvo:TrustedExecutionEnvironments a owl:Class ;
    rdfs:label "Trusted Execution Environments"@en ;
    dct:created "2022-08-17"^^xsd:date ;
    dct:creator "Harshvardhan J. Pandit"^^xsd:string ;
    dct:description "Use of cryptographic methods to restrict access and execution to trusted parties and code within a dedicated execution environment"@en ;
    dct:source <https://www.enisa.europa.eu/publications/data-protection-engineering> ;
    rdfs:isDefinedBy dpvo: ;
    rdfs:subClassOf dpvo:CryptographicMethods ;
    sw:term_status "accepted"@en .

dpvo:TrustedThirdPartyUtilisation a owl:Class ;
    rdfs:label "Trusted Third Party Utilisation"@en ;
    dct:created "2022-08-17"^^xsd:date ;
    dct:creator "Harshvardhan J. Pandit"^^xsd:string ;
    dct:description "Utilisation of a trusted third party to provide or carry out a measure"@en ;
    dct:source <https://www.enisa.europa.eu/publications/data-pseudonymisation-advanced-techniques-and-use-cases> ;
    rdfs:isDefinedBy dpvo: ;
    rdfs:subClassOf dpvo:SecurityProcedure ;
    sw:term_status "accepted"@en .

dpvo:UninformedConsent a owl:Class ;
    rdfs:label "Uninformed Consent"@en ;
    dct:created "2022-06-21"^^xsd:date ;
    dct:creator "Georg P Krog"^^xsd:string,
        "Harshvardhan J. Pandit"^^xsd:string,
        "Julian Flake"^^xsd:string,
        "Paul Ryan"^^xsd:string ;
    dct:description "Consent that is uninformed i.e. without requirement to provide sufficient information to make a consenting decision"@en ;
    rdfs:isDefinedBy dpvo: ;
    rdfs:subClassOf dpvo:Consent ;
    sw:term_status "accepted"@en .

dpvo:Unlawful a owl:NamedIndividual,
        dpvo:Lawfulness ;
    rdfs:label "Unlawful"@en ;
    dct:created "2022-10-19"^^xsd:date ;
    dct:creator "Harshvardhan J. Pandit"^^xsd:string ;
    dct:description "State of being unlawful or legally non-compliant"@en ;
    rdfs:isDefinedBy dpvo: ;
    sw:term_status "accepted"@en .

dpvo:UntilEventDuration a owl:Class ;
    rdfs:label "Until Event Duration"@en ;
    dct:created "2022-06-15"^^xsd:date ;
    dct:creator "Harshvardhan J. Pandit"^^xsd:string ;
    dct:description "Duration that takes place until a specific event occurs e.g. Account Closure"@en ;
    dct:modified "2020-10-05"^^xsd:date ;
    rdfs:isDefinedBy dpvo: ;
    rdfs:subClassOf dpvo:Duration ;
    sw:term_status "modified"@en .

dpvo:UntilTimeDuration a owl:Class ;
    rdfs:label "Until Time Duration"@en ;
    dct:created "2022-06-15"^^xsd:date ;
    dct:creator "Harshvardhan J. Pandit"^^xsd:string ;
    dct:description "Duration that has a fixed end date e.g. 2022-12-31"@en ;
    dct:modified "2020-10-05"^^xsd:date ;
    rdfs:isDefinedBy dpvo: ;
    rdfs:subClassOf dpvo:Duration ;
    sw:term_status "modified"@en .

dpvo:UnverifiedData a owl:Class ;
    rdfs:label "Unverified Data"@en ;
    dct:created "2022-11-02"^^xsd:date ;
    dct:creator "Harshvardhan J. Pandit"^^xsd:string ;
    dct:description "Data that has not been verified in terms of accuracy, inconsistency, or quality"@en ;
    rdfs:isDefinedBy dpvo: ;
    rdfs:subClassOf dpvo:Data ;
    sw:term_status "accepted"@en .

dpvo:UsageControl a owl:Class ;
    rdfs:label "Usage Control"@en ;
    dct:created "2022-08-17"^^xsd:date ;
    dct:creator "Harshvardhan J. Pandit"^^xsd:string ;
    dct:description "Management of usage, which is intended to be broader than access control and may cover trust, digital rights, or other relevant controls"@en ;
    dct:source <https://www.enisa.europa.eu/publications/reference-incident-classification-taxonomy/> ;
    rdfs:isDefinedBy dpvo: ;
    rdfs:subClassOf dpvo:AccessControlMethod ;
    sw:term_status "accepted"@en .

dpvo:UseSyntheticData a owl:Class ;
    rdfs:label "Use of Synthetic Data"@en ;
    dct:created "2022-08-17"^^xsd:date ;
    dct:creator "Harshvardhan J. Pandit"^^xsd:string ;
    dct:description "Use of synthetic data to preserve privacy, security, or other effects and side-effects"@en ;
    dct:source <https://www.enisa.europa.eu/publications/data-protection-engineering> ;
    rdfs:isDefinedBy dpvo: ;
    rdfs:subClassOf dpvo:SecurityMethod ;
    sw:term_status "accepted"@en .

dpvo:User a owl:Class ;
    rdfs:label "User"@en ;
    dct:created "2022-04-06"^^xsd:date ;
    dct:creator "Beatriz Esteves"^^xsd:string,
        "Georg P. Krog"^^xsd:string,
        "Harshvardhan J. Pandit"^^xsd:string,
        "Julian Flake"^^xsd:string,
        "Paul Ryan"^^xsd:string ;
    dct:description "Data subjects that use service(s)"@en ;
    rdfs:isDefinedBy dpvo: ;
    rdfs:subClassOf dpvo:DataSubject ;
    sw:term_status "accepted"@en .

dpvo:UserInterfacePersonalisation a owl:Class ;
    rdfs:label "User Interface Personalisation"@en ;
    dct:created "2019-04-05"^^xsd:date ;
    dct:creator "Axel Polleres"^^xsd:string,
        "Elmar Kiesling"^^xsd:string,
        "Fajar Ekaputra"^^xsd:string,
        "Harshvardhan J. Pandit"^^xsd:string,
        "Javier Fernandez"^^xsd:string,
        "Simon Steyskal"^^xsd:string ;
    dct:description "Purposes associated with personalisation of interfaces presented to the user"@en ;
    rdfs:comment "Examples of user-interface personalisation include changing the language to match the locale"@en ;
    rdfs:isDefinedBy dpvo: ;
    rdfs:subClassOf dpvo:ServicePersonalisation ;
    sw:term_status "accepted"@en .

dpvo:VariableLocation a owl:Class ;
    rdfs:label "Variable Location"@en ;
    dct:created "2022-06-15"^^xsd:date ;
    dct:creator "Harshvardhan J. Pandit"^^xsd:string ;
    dct:description "Location that is known but is variable e.g. somewhere within a given area"@en ;
    dct:modified "2020-10-05"^^xsd:date ;
    rdfs:isDefinedBy dpvo: ;
    rdfs:subClassOf dpvo:LocationFixture ;
    sw:term_status "modified"@en .

dpvo:VendorPayment a owl:Class ;
    rdfs:label "Vendor Payment"@en ;
    dct:created "2021-09-01"^^xsd:date ;
    dct:creator "David Hickey"^^xsd:string,
        "Georg P Krog"^^xsd:string,
        "Harshvardhan J. Pandit"^^xsd:string,
        "Paul Ryan"^^xsd:string ;
    dct:description "Purposes associated with managing payment of vendors"@en ;
    dct:source <https://www.privacycommission.be/nl/model-voor-een-register-van-de-verwerkingsactiviteiten> ;
    rdfs:isDefinedBy dpvo: ;
    rdfs:subClassOf dpvo:VendorManagement ;
    sw:term_status "accepted"@en .

dpvo:VendorRecordsManagement a owl:Class ;
    rdfs:label "Vendor Records Management"@en ;
    dct:created "2021-09-01"^^xsd:date ;
    dct:creator "David Hickey"^^xsd:string,
        "Georg P Krog"^^xsd:string,
        "Harshvardhan J. Pandit"^^xsd:string,
        "Paul Ryan"^^xsd:string ;
    dct:description "Purposes associated with managing records and orders related to vendors"@en ;
    dct:source <https://www.privacycommission.be/nl/model-voor-een-register-van-de-verwerkingsactiviteiten> ;
    rdfs:isDefinedBy dpvo: ;
    rdfs:subClassOf dpvo:VendorManagement ;
    sw:term_status "accepted"@en .

dpvo:VendorSelectionAssessment a owl:Class ;
    rdfs:label "Vendor Selection Assessment"@en ;
    dct:created "2021-09-01"^^xsd:date ;
    dct:creator "David Hickey"^^xsd:string,
        "Georg P Krog"^^xsd:string,
        "Harshvardhan J. Pandit"^^xsd:string,
        "Paul Ryan"^^xsd:string ;
    dct:description "Purposes associated with managing selection, assessment, and evaluation related to vendors"@en ;
    dct:source <https://www.privacycommission.be/nl/model-voor-een-register-van-de-verwerkingsactiviteiten> ;
    rdfs:isDefinedBy dpvo: ;
    rdfs:subClassOf dpvo:VendorManagement ;
    sw:term_status "accepted"@en .

dpvo:VerifiedData a owl:Class ;
    rdfs:label "Verified Data"@en ;
    dct:created "2022-11-02"^^xsd:date ;
    dct:creator "Harshvardhan J. Pandit"^^xsd:string ;
    dct:description "Data that has been verified in terms of accuracy, inconsistency, or quality"@en ;
    rdfs:isDefinedBy dpvo: ;
    rdfs:subClassOf dpvo:Data ;
    sw:term_status "accepted"@en .

dpvo:VirtualisationSecurity a owl:Class ;
    rdfs:label "Virtualisation Security"@en ;
    dct:created "2022-08-17"^^xsd:date ;
    dct:creator "Harshvardhan J. Pandit"^^xsd:string ;
    dct:description "Security implemented at or through virtualised environments"@en ;
    dct:source <https://www.enisa.europa.eu/publications/reference-incident-classification-taxonomy/> ;
    rdfs:isDefinedBy dpvo: ;
    rdfs:subClassOf dpvo:SecurityMethod ;
    sw:term_status "accepted"@en .

dpvo:Visitor a owl:Class ;
    rdfs:label "Visitor"@en ;
    dct:created "2022-04-06"^^xsd:date ;
    dct:creator "Beatriz Esteves"^^xsd:string,
        "Georg P. Krog"^^xsd:string,
        "Harshvardhan J. Pandit"^^xsd:string,
        "Julian Flake"^^xsd:string,
        "Paul Ryan"^^xsd:string ;
    dct:description "Data subjects that are temporary visitors"@en ;
    rdfs:isDefinedBy dpvo: ;
    rdfs:subClassOf dpvo:DataSubject ;
    sw:term_status "accepted"@en .

dpvo:VitalInterestOfDataSubject a owl:Class ;
    rdfs:label "Vital Interest of Data Subject"@en ;
    dct:created "2021-04-21"^^xsd:date ;
    dct:creator "Georg P Krog"^^xsd:string,
        "Harshvardhan J. Pandit"^^xsd:string,
        "Paul Ryan"^^xsd:string ;
    dct:description "Processing is necessary or required to protect vital interests of a data subject"@en ;
    rdfs:isDefinedBy dpvo: ;
    rdfs:subClassOf dpvo:VitalInterestOfNaturalPerson ;
    sw:term_status "accepted"@en .

dpvo:VulnerabilityTestingMethods a owl:Class ;
    rdfs:label "Vulnerability Testing Methods"@en ;
    dct:created "2022-08-17"^^xsd:date ;
    dct:creator "Harshvardhan J. Pandit"^^xsd:string ;
    dct:description "Methods that assess or discover vulnerabilities in a system"@en ;
    dct:source <https://www.enisa.europa.eu/publications/reference-incident-classification-taxonomy/> ;
    rdfs:isDefinedBy dpvo: ;
    rdfs:subClassOf dpvo:SecurityMethod ;
    sw:term_status "accepted"@en .

dpvo:WebBrowserSecurity a owl:Class ;
    rdfs:label "WebBrowser Security"@en ;
    dct:created "2022-08-17"^^xsd:date ;
    dct:creator "Harshvardhan J. Pandit"^^xsd:string ;
    dct:description "Security implemented at or over web browsers"@en ;
    dct:source <https://www.enisa.europa.eu/publications/reference-incident-classification-taxonomy/> ;
    rdfs:isDefinedBy dpvo: ;
    rdfs:subClassOf dpvo:SecurityMethod ;
    sw:term_status "accepted"@en .

dpvo:WebSecurityProtocols a owl:Class ;
    rdfs:label "Web Security Protocols"@en ;
    dct:created "2022-08-17"^^xsd:date ;
    dct:creator "Harshvardhan J. Pandit"^^xsd:string ;
    dct:description "Security implemented at or over web-based protocols"@en ;
    dct:source <https://www.enisa.europa.eu/publications/reference-incident-classification-taxonomy/> ;
    rdfs:isDefinedBy dpvo: ;
    rdfs:subClassOf dpvo:SecurityMethod ;
    sw:term_status "accepted"@en .

dpvo:WirelessSecurityProtocols a owl:Class ;
    rdfs:label "Wireless Security Protocols"@en ;
    dct:created "2022-08-17"^^xsd:date ;
    dct:creator "Harshvardhan J. Pandit"^^xsd:string ;
    dct:description "Security implemented at or over wireless communication protocols"@en ;
    dct:source <https://www.enisa.europa.eu/publications/reference-incident-classification-taxonomy/> ;
    rdfs:isDefinedBy dpvo: ;
    rdfs:subClassOf dpvo:SecurityMethod ;
    sw:term_status "accepted"@en .

dpvo:WithinDevice a owl:Class ;
    rdfs:label "Within Device"@en ;
    dct:created "2022-06-15"^^xsd:date ;
    dct:creator "Harshvardhan J. Pandit"^^xsd:string ;
    dct:description "Location is local and entirely within a device, such as a smartphone"@en ;
    dct:modified "2020-10-05"^^xsd:date ;
    rdfs:isDefinedBy dpvo: ;
    rdfs:subClassOf dpvo:LocalLocation ;
    sw:term_status "modified"@en .

dpvo:WithinPhysicalEnvironment a owl:Class ;
    rdfs:label "Within Physical Environment"@en ;
    dct:created "2020-10-06"^^xsd:date ;
    dct:creator "Harshvardhan J. Pandit"^^xsd:string ;
    dct:description "Location is local and entirely within a physical environment, such as a room"@en ;
    rdfs:isDefinedBy dpvo: ;
    rdfs:subClassOf dpvo:LocalLocation ;
    sw:term_status "accepted"@en .

dpvo:WithinVirtualEnvironment a owl:Class ;
    rdfs:label "Within Virtual Environment"@en ;
    dct:created "2020-10-06"^^xsd:date ;
    dct:creator "Harshvardhan J. Pandit"^^xsd:string ;
    dct:description "Location is local and entirely within a virtual environment, such as a shared network directory"@en ;
    rdfs:isDefinedBy dpvo: ;
    rdfs:subClassOf dpvo:LocalLocation ;
    sw:term_status "accepted"@en .

dpvo:ZeroKnowledgeAuthentication a owl:Class ;
    rdfs:label "Zero Knowledge Authentication"@en ;
    dct:created "2022-08-17"^^xsd:date ;
    dct:creator "Harshvardhan J. Pandit"^^xsd:string ;
    dct:description "Authentication using Zero-Knowledge proofs"@en ;
    dct:source <https://www.enisa.europa.eu/publications/data-protection-engineering> ;
    rdfs:isDefinedBy dpvo: ;
    rdfs:subClassOf dpvo:AuthenticationProtocols,
        dpvo:CryptographicMethods ;
    sw:term_status "accepted"@en .

dpvo:hasActivityStatus a rdf:Property,
        owl:ObjectProperty ;
    rdfs:label "has activity status"@en ;
    dct:created "2022-05-18"^^xsd:date ;
    dct:creator "Harshvardhan J. Pandit"^^xsd:string ;
    dct:description "Indicates the status of activity of specified concept"@en ;
    rdfs:domain owl:Thing ;
    rdfs:isDefinedBy dpvo: ;
    rdfs:range dpvo:ActivityStatus ;
    rdfs:subPropertyOf dpvo:hasStatus ;
    sw:term_status "accepted"@en .

dpvo:hasAddress a rdf:Property,
        owl:ObjectProperty ;
    rdfs:label "has address"@en ;
    dct:created "2020-11-04"^^xsd:date ;
    dct:creator "Beatriz Esteves"^^xsd:string,
        "Georg P Krog"^^xsd:string,
        "Harshvardhan J.Pandit"^^xsd:string,
        "Paul Ryan"^^xsd:string ;
    dct:description "Specifies address of a legal entity such as street address or pin code"@en ;
    rdfs:domain dpvo:Entity ;
    rdfs:isDefinedBy dpvo: ;
    rdfs:range owl:Thing ;
    sw:term_status "accepted"@en .

dpvo:hasAlgorithmicLogic a rdf:Property,
        owl:ObjectProperty ;
    rdfs:label "has algorithmic logic"@en ;
    dct:created "2020-11-04"^^xsd:date ;
    dct:creator "Georg P. Krog"^^xsd:string,
        "Harshvardhan J. Pandit"^^xsd:string,
        "Paul Ryan"^^xsd:string ;
    dct:description "Indicates the logic used in processing such as for automated decision making"@en ;
    dct:modified "2022-06-15"^^xsd:date ;
    rdfs:domain owl:Thing ;
    rdfs:isDefinedBy dpvo: ;
    rdfs:range dpvo:AlgorithmicLogic ;
    sw:term_status "changed"@en .

dpvo:hasApplicableLaw a rdf:Property,
        owl:ObjectProperty ;
    rdfs:label "has applicable law"@en ;
    dct:created "2022-01-19"^^xsd:date ;
    dct:creator "Harshvardhan J. Pandit"^^xsd:string ;
    dct:description "Indicates applicability of a Law"@en ;
    rdfs:domain owl:Thing ;
    rdfs:isDefinedBy dpvo: ;
    rdfs:range dpvo:Law ;
    sw:term_status "accepted"@en .

dpvo:hasAuditStatus a rdf:Property,
        owl:ObjectProperty ;
    rdfs:label "has audit status"@en ;
    dct:created "2022-06-22"^^xsd:date ;
    dct:creator "Harshvardhan J. Pandit"^^xsd:string ;
    dct:description "Indicates the status of audit associated with specified concept"@en ;
    rdfs:domain owl:Thing ;
    rdfs:isDefinedBy dpvo: ;
    rdfs:range dpvo:AuditStatus ;
    rdfs:subPropertyOf dpvo:hasStatus ;
    sw:term_status "accepted"@en .

dpvo:hasAuthority a rdf:Property,
        owl:ObjectProperty ;
    rdfs:label "has authority"@en ;
    dct:created "2022-01-19"^^xsd:date ;
    dct:creator "Georg P Krog"^^xsd:string,
        "Harshvardhan J. Pandit"^^xsd:string ;
    dct:description "Indicates applicability of authority for a jurisdiction"@en ;
    rdfs:domain owl:Thing ;
    rdfs:isDefinedBy dpvo: ;
    rdfs:range dpvo:Authority ;
    sw:term_status "accepted"@en .

dpvo:hasConsentStatus a rdf:Property,
        owl:ObjectProperty ;
    rdfs:label "has consent status"@en ;
    dct:created "2022-06-21"^^xsd:date ;
    dct:creator "Georg P Krog"^^xsd:string,
        "Harshvardhan J. Pandit"^^xsd:string,
        "Julian Flake"^^xsd:string,
        "Paul Ryan"^^xsd:string ;
    dct:description "Specifies the state or status of consent"@en ;
    rdfs:domain owl:Thing ;
    rdfs:isDefinedBy dpvo: ;
    rdfs:range dpvo:ConsentStatus ;
    sw:term_status "accepted"@en .

dpvo:hasContact a rdf:Property,
        owl:ObjectProperty ;
    rdfs:label "has contact"@en ;
    dct:created "2020-11-04"^^xsd:date ;
    dct:creator "Beatriz Esteves"^^xsd:string,
        "Georg P Krog"^^xsd:string,
        "Harshvardhan J.Pandit"^^xsd:string,
        "Paul Ryan"^^xsd:string ;
    dct:description "Specifies contact details of a legal entity such as phone  or email"@en ;
    rdfs:domain dpvo:Entity ;
    rdfs:isDefinedBy dpvo: ;
    rdfs:range owl:Thing ;
    sw:term_status "accepted"@en .

dpvo:hasContext a rdf:Property,
        owl:ObjectProperty ;
    rdfs:label "has context"@en ;
    dct:created "2019-04-05"^^xsd:date ;
    dct:description "Indicates a purpose is restricted to the specified context(s)"@en ;
    rdfs:domain owl:Thing ;
    rdfs:isDefinedBy dpvo: ;
    rdfs:range dpvo:Context ;
    sw:term_status "accepted"@en .

dpvo:hasDataExporter a rdf:Property,
        owl:ObjectProperty ;
    rdfs:label "has data exporter"@en ;
    dct:created "2022-02-09"^^xsd:date ;
    dct:creator "Georg P. Krog"^^xsd:string,
        "Harshvardhan J. Pandit"^^xsd:string,
        "Paul Ryan"^^xsd:string ;
    dct:description "Indiciates inclusion or applicability of a LegalEntity in the role of Data Exporter"@en ;
    rdfs:domain owl:Thing ;
    rdfs:isDefinedBy dpvo: ;
    rdfs:range dpvo:DataExporter ;
    rdfs:subPropertyOf dpvo:hasEntity ;
    sw:term_status "accepted"@en .

dpvo:hasDataImporter a rdf:Property,
        owl:ObjectProperty ;
    rdfs:label "has data importer"@en ;
    dct:created "2022-02-09"^^xsd:date ;
    dct:creator "Georg P. Krog"^^xsd:string,
        "Harshvardhan J. Pandit"^^xsd:string,
        "Paul Ryan"^^xsd:string ;
    dct:description "Indiciates inclusion or applicability of a LegalEntity in the role of Data Importer"@en ;
    rdfs:domain owl:Thing ;
    rdfs:isDefinedBy dpvo: ;
    rdfs:range dpvo:DataImporter ;
    rdfs:subPropertyOf dpvo:hasRecipient ;
    sw:term_status "accepted"@en .

dpvo:hasDataProcessor a rdf:Property,
        owl:ObjectProperty ;
    rdfs:label "has data processor"@en ;
    dct:created "2022-02-09"^^xsd:date ;
    dct:creator "Georg P. Krog"^^xsd:string,
        "Harshvardhan J. Pandit"^^xsd:string,
        "Paul Ryan"^^xsd:string ;
    dct:description "Indiciates inclusion or applicability of a Data Processor"@en ;
    rdfs:domain owl:Thing ;
    rdfs:isDefinedBy dpvo: ;
    rdfs:range dpvo:DataProcessor ;
    rdfs:subPropertyOf dpvo:hasRecipient ;
    sw:term_status "accepted"@en .

dpvo:hasDataProtectionOfficer a rdf:Property,
        owl:ObjectProperty ;
    rdfs:label "has data protection officer"@en ;
    dct:created "2022-03-02"^^xsd:date ;
    dct:creator "Paul Ryan"^^xsd:string,
        "Rob Brennan"^^xsd:string ;
    dct:description "Specifices an associated data protection officer"@en ;
    rdfs:domain owl:Thing ;
    rdfs:isDefinedBy dpvo: ;
    rdfs:range dpvo:DataProtectionOfficer ;
    rdfs:subPropertyOf dpvo:hasRepresentative ;
    sw:term_status "accepted"@en .

dpvo:hasDataSource a rdf:Property,
        owl:ObjectProperty ;
    rdfs:label "has data source"@en ;
    dct:created "2020-11-04"^^xsd:date ;
    dct:creator "Georg P. Krog"^^xsd:string,
        "Harshvardhan J. Pandit"^^xsd:string,
        "Paul Ryan"^^xsd:string ;
    dct:description "Indicates the source or origin of data being processed"@en ;
    rdfs:domain owl:Thing ;
    rdfs:isDefinedBy dpvo: ;
    rdfs:range dpvo:DataSource ;
    sw:term_status "accepted"@en .

dpvo:hasDataSubject a rdf:Property,
        owl:ObjectProperty ;
    rdfs:label "has data subject"@en ;
    dct:created "2019-04-04"^^xsd:date ;
    dct:creator "Axel Polleres"^^xsd:string,
        "Bud Bruegger"^^xsd:string,
        "Harshvardhan J. Pandit"^^xsd:string,
        "Javier Fernández"^^xsd:string,
        "Mark Lizar"^^xsd:string ;
    dct:description "Indicates association with Data Subject"@en ;
    dct:modified "2020-11-04"^^xsd:date ;
    rdfs:domain owl:Thing ;
    rdfs:isDefinedBy dpvo: ;
    rdfs:range dpvo:DataSubject ;
    rdfs:subPropertyOf dpvo:hasEntity ;
    sw:term_status "accepted"@en .

dpvo:hasDataSubjectScale a rdf:Property,
        owl:ObjectProperty ;
    rdfs:label "has data subject scale"@en ;
    dct:created "2022-06-22"^^xsd:date ;
    dct:creator "Harshvardhan J. Pandit"^^xsd:string ;
    dct:description "Indicates the scale of data subjects"@en ;
    rdfs:domain owl:Thing ;
    rdfs:isDefinedBy dpvo: ;
    rdfs:range dpvo:DataSubjectScale ;
    rdfs:subPropertyOf dpvo:hasScale ;
    sw:term_status "accepted"@en .

dpvo:hasDataVolume a rdf:Property,
        owl:ObjectProperty ;
    rdfs:label "has data volume"@en ;
    dct:created "2022-06-22"^^xsd:date ;
    dct:creator "Harshvardhan J. Pandit"^^xsd:string ;
    dct:description "Indicates the volume of data"@en ;
    rdfs:domain owl:Thing ;
    rdfs:isDefinedBy dpvo: ;
    rdfs:range dpvo:DataVolume ;
    rdfs:subPropertyOf dpvo:hasScale ;
    sw:term_status "accepted"@en .

dpvo:hasDuration a rdf:Property,
        owl:ObjectProperty ;
    rdfs:label "has duration"@en ;
    dct:created "2019-04-05"^^xsd:date ;
    dct:creator "Axel Polleres"^^xsd:string,
        "Harshvardhan J. Pandit"^^xsd:string,
        "Mark Lizar"^^xsd:string,
        "Rob Brennan"^^xsd:string ;
    dct:description "Indicates information about duration"@en ;
    dct:source <https://specialprivacy.ercim.eu/> ;
    rdfs:domain owl:Thing ;
    rdfs:isDefinedBy dpvo: ;
    rdfs:range dpvo:Duration ;
    sw:term_status "accepted"@en .

dpvo:hasFrequency a rdf:Property,
        owl:ObjectProperty ;
    rdfs:label "has frequency"@en ;
    dct:created "2022-02-16"^^xsd:date ;
    dct:creator "Harshvardhan J. Pandit"^^xsd:string ;
    dct:description "Indicates the frequency with which something takes place"@en ;
    rdfs:domain owl:Thing ;
    rdfs:isDefinedBy dpvo: ;
    rdfs:range dpvo:Frequency ;
    sw:term_status "accepted"@en .

dpvo:hasGeographicCoverage a rdf:Property,
        owl:ObjectProperty ;
    rdfs:label "has geographic coverage"@en ;
    dct:created "2022-06-22"^^xsd:date ;
    dct:creator "Harshvardhan J. Pandit"^^xsd:string ;
    dct:description "Indicate the geographic coverage (of specified context)"@en ;
    rdfs:domain owl:Thing ;
    rdfs:isDefinedBy dpvo: ;
    rdfs:range dpvo:GeographicCoverage ;
    rdfs:subPropertyOf dpvo:hasScale ;
    sw:term_status "accepted"@en .

dpvo:hasHumanInvolvement a rdf:Property,
        owl:ObjectProperty ;
    rdfs:label "has human involvement"@en ;
    dct:created "2020-11-04"^^xsd:date ;
    dct:creator "Georg P. Krog"^^xsd:string,
        "Harshvardhan J. Pandit"^^xsd:string,
        "Paul Ryan"^^xsd:string ;
    dct:description "Indicates Involvement of humans in processing such as within automated decision making process"@en ;
    rdfs:comment "Human involvement is also relevant to 'human in the loop'"@en ;
    rdfs:domain owl:Thing ;
    rdfs:isDefinedBy dpvo: ;
    rdfs:range dpvo:HumanInvolvement ;
    sw:term_status "accepted"@en .

dpvo:hasIdentifier a rdf:Property,
        owl:ObjectProperty ;
    rdfs:label "has identifier"@en ;
    dct:created "2020-11-25"^^xsd:date ;
    dct:creator "Beatriz Esteves"^^xsd:string,
        "Georg P Krog"^^xsd:string,
        "Harshvardhan J.Pandit"^^xsd:string,
        "Paul Ryan"^^xsd:string ;
    dct:description "Indicates an identifier associated for identification or reference"@en ;
    rdfs:domain owl:Thing ;
    rdfs:isDefinedBy dpvo: ;
    rdfs:range owl:Thing ;
    sw:term_status "accepted"@en .

dpvo:hasImpact a rdf:Property,
        owl:ObjectProperty ;
    rdfs:label "has impact"@en ;
    dct:created "2022-05-18"^^xsd:date ;
    dct:creator "Beatriz Esteves"^^xsd:string,
        "Fajar Ekaputra"^^xsd:string,
        "Georg P Krog"^^xsd:string,
        "Harshvardhan J. Pandit"^^xsd:string,
        "Julian Flake"^^xsd:string ;
    dct:description "Indicates impact(s) possible or arising as consequences from specified concept"@en ;
    rdfs:domain owl:Thing ;
    rdfs:isDefinedBy dpvo: ;
    rdfs:range dpvo:Impact ;
    rdfs:subPropertyOf dpvo:hasConsequence ;
    sw:term_status "accepted"@en .

dpvo:hasImpactOn a rdf:Property,
        owl:ObjectProperty ;
    rdfs:label "has impact on"@en ;
    dct:created "2022-05-18"^^xsd:date ;
    dct:creator "Beatriz Esteves"^^xsd:string,
        "Fajar Ekaputra"^^xsd:string,
        "Georg P Krog"^^xsd:string,
        "Harshvardhan J. Pandit"^^xsd:string,
        "Julian Flake"^^xsd:string ;
    dct:description "Indicates the thing (e.g. plan, process, or entity) affected by an impact"@en ;
    rdfs:domain dpvo:Impact ;
    rdfs:isDefinedBy dpvo: ;
    rdfs:range owl:Thing ;
    rdfs:subPropertyOf dpvo:hasConsequenceOn ;
    sw:term_status "accepted"@en .

dpvo:hasIndicationMethod a rdf:Property,
        owl:ObjectProperty ;
    rdfs:label "has indication method"@en ;
    dct:created "2022-06-21"^^xsd:date ;
    dct:creator "Georg P Krog"^^xsd:string,
        "Harshvardhan J. Pandit"^^xsd:string,
        "Julian Flake"^^xsd:string,
        "Paul Ryan"^^xsd:string ;
    dct:description "Specifies the method by which an entity has indicated the specific context"@en ;
    rdfs:domain owl:Thing ;
    rdfs:isDefinedBy dpvo: ;
    sw:term_status "accepted"@en .

dpvo:hasJointDataControllers a rdf:Property,
        owl:ObjectProperty ;
    rdfs:label "has joint data controllers"@en ;
    dct:created "2022-02-09"^^xsd:date ;
    dct:creator "Georg P. Krog"^^xsd:string,
        "Harshvardhan J. Pandit"^^xsd:string,
        "Paul Ryan"^^xsd:string ;
    dct:description "Indicates inclusion or applicability of a Joint Data Controller"@en ;
    rdfs:domain owl:Thing ;
    rdfs:isDefinedBy dpvo: ;
    rdfs:range dpvo:JointDataControllers ;
    rdfs:subPropertyOf dpvo:hasDataController ;
    sw:term_status "accepted"@en .

dpvo:hasJurisdiction a rdf:Property,
        owl:ObjectProperty ;
    rdfs:label "has jurisdiction"@en ;
    dct:created "2022-01-19"^^xsd:date ;
    dct:creator "Harshvardhan J. Pandit"^^xsd:string ;
    dct:description "Indicates applicability of specified jurisdiction"@en ;
    rdfs:domain owl:Thing ;
    rdfs:isDefinedBy dpvo: ;
    rdfs:range dpvo:Location ;
    sw:term_status "accepted"@en .

dpvo:hasJustification a rdf:Property,
        owl:ObjectProperty ;
    rdfs:label "has justification"@en ;
    dct:created "2022-06-15"^^xsd:date ;
    dct:creator "Harshvardhan J. Pandit"^^xsd:string ;
    dct:description "Indicates a justification for specified concept or context"@en ;
    rdfs:domain owl:Thing ;
    rdfs:isDefinedBy dpvo: ;
    rdfs:range dpvo:Justification ;
    sw:term_status "accepted"@en .

dpvo:hasLawfulness a rdf:Property,
        owl:ObjectProperty ;
    rdfs:label "has lawfulness"@en ;
    dct:created "2022-10-22"^^xsd:date ;
    dct:creator "Harshvardhan J. Pandit"^^xsd:string ;
    dct:description "Indicates the status of being lawful or legally compliant"@en ;
    rdfs:domain owl:Thing ;
    rdfs:isDefinedBy dpvo: ;
    rdfs:range dpvo:Lawfulness ;
    rdfs:subPropertyOf dpvo:hasComplianceStatus ;
    sw:term_status "accepted"@en .

dpvo:hasLegalBasis a rdf:Property,
        owl:ObjectProperty ;
    rdfs:label "has legal basis"@en ;
    dct:created "2019-04-04"^^xsd:date ;
    dct:creator "Axel Polleres"^^xsd:string,
        "Javier Fernández"^^xsd:string ;
    dct:description "Indicates use or applicability of a Legal Basis"@en ;
    dct:modified "2020-11-04"^^xsd:date ;
    rdfs:domain owl:Thing ;
    rdfs:isDefinedBy dpvo: ;
    rdfs:range dpvo:LegalBasis ;
    sw:term_status "accepted"@en .

dpvo:hasLikelihood a rdf:Property,
        owl:ObjectProperty ;
    rdfs:label "has likelihood"@en ;
    dct:created "2022-07-20"^^xsd:date ;
    dct:creator "Georg P Krog"^^xsd:string,
        "Harshvardhan J. Pandit"^^xsd:string,
        "Julian Flake"^^xsd:string,
        "Paul Ryan"^^xsd:string ;
    dct:description "Indicates the likelihood associated with a concept"@en ;
    rdfs:domain owl:Thing ;
    rdfs:isDefinedBy dpvo: ;
    rdfs:range dpvo:Likelihood ;
    sw:term_status "accepted"@en .

dpvo:hasName a rdf:Property,
        owl:ObjectProperty ;
    rdfs:label "has name"@en ;
    dct:created "2020-11-04"^^xsd:date ;
    dct:creator "Beatriz Esteves"^^xsd:string,
        "Georg P Krog"^^xsd:string,
        "Harshvardhan J.Pandit"^^xsd:string,
        "Paul Ryan"^^xsd:string ;
    dct:description "Specifies name of a legal entity"@en ;
    rdfs:domain dpvo:Entity ;
    rdfs:isDefinedBy dpvo: ;
    rdfs:range owl:Thing ;
    sw:term_status "accepted"@en .

dpvo:hasNotice a rdf:Property,
        owl:ObjectProperty ;
    rdfs:label "has notice"@en ;
    dct:created "2022-06-22"^^xsd:date ;
    dct:creator "Georg P Krog"^^xsd:string,
        "Harshvardhan J. Pandit"^^xsd:string,
        "Julian Flake"^^xsd:string,
        "Paul Ryan"^^xsd:string ;
    dct:description "Indicates the use or applicability of a Notice for the specified context"@en ;
    rdfs:domain owl:Thing ;
    rdfs:isDefinedBy dpvo: ;
    rdfs:range dpvo:Notice ;
    rdfs:subPropertyOf dpvo:hasOrganisationalMeasure ;
    sw:term_status "accepted"@en .

dpvo:hasObligation a rdf:Property,
        owl:ObjectProperty ;
    rdfs:label "has obligation"@en ;
    dct:created "2022-10-19"^^xsd:date ;
    dct:creator "Beatriz Esteves"^^xsd:string,
        "Georg P Krog"^^xsd:string,
        "Harshvardhan J. Pandit"^^xsd:string,
        "Paul Ryan"^^xsd:string ;
    dct:description "Specifying applicability or inclusion of an obligation rule within specified context"@en ;
    rdfs:domain dpvo:Context ;
    rdfs:isDefinedBy dpvo: ;
    rdfs:range dpvo:Obligation ;
    rdfs:subPropertyOf dpvo:hasRule ;
    sw:term_status "accepted"@en .

dpvo:hasOutcome a rdf:Property,
        owl:ObjectProperty ;
    rdfs:label "has outcome"@en ;
    dct:created "2022-05-18"^^xsd:date ;
    dct:creator "Harshvardhan J. Pandit"^^xsd:string ;
    dct:description "Indicates an outcome of specified concept or context"@en ;
    rdfs:domain owl:Thing ;
    rdfs:isDefinedBy dpvo: ;
    rdfs:range owl:Thing ;
    sw:term_status "accepted"@en .

dpvo:hasPermission a rdf:Property,
        owl:ObjectProperty ;
    rdfs:label "has permission"@en ;
    dct:created "2022-10-19"^^xsd:date ;
    dct:creator "Beatriz Esteves"^^xsd:string,
        "Georg P Krog"^^xsd:string,
        "Harshvardhan J. Pandit"^^xsd:string,
        "Paul Ryan"^^xsd:string ;
    dct:description "Specifying applicability or inclusion of a permission rule within specified context"@en ;
    rdfs:domain dpvo:Context ;
    rdfs:isDefinedBy dpvo: ;
    rdfs:range dpvo:Permission ;
    rdfs:subPropertyOf dpvo:hasRule ;
    sw:term_status "accepted"@en .

dpvo:hasPersonalData a rdf:Property,
        owl:ObjectProperty ;
    rdfs:label "has personal data"@en ;
    dct:created "2022-01-19"^^xsd:date ;
    dct:creator "Harshvardhan J. Pandit"^^xsd:string ;
    dct:description "Indicates association with Personal Data"@en ;
    rdfs:domain owl:Thing ;
    rdfs:isDefinedBy dpvo: ;
    rdfs:range dpvo:PersonalData ;
    rdfs:subPropertyOf dpvo:hasData ;
    sw:term_status "accepted"@en .

dpvo:hasPersonalDataHandling a rdf:Property,
        owl:ObjectProperty ;
    rdfs:label "has personal data handling"@en ;
    dct:created "2022-01-19"^^xsd:date ;
    dct:creator "Georg P Krog"^^xsd:string,
        "Harshvardhan J. Pandit"^^xsd:string ;
    dct:description "Indicates association with Personal Data Handling"@en ;
    rdfs:domain owl:Thing ;
    rdfs:isDefinedBy dpvo: ;
    rdfs:range dpvo:PersonalDataHandling ;
    sw:term_status "accepted"@en .

dpvo:hasPolicy a rdf:Property,
        owl:ObjectProperty ;
    rdfs:label "has policy"@en ;
    dct:created "2022-01-26"^^xsd:date ;
    dct:creator "Harshvardhan J. Pandit"^^xsd:string ;
    dct:description "Indicates policy applicable or used"@en ;
    rdfs:domain owl:Thing ;
    rdfs:isDefinedBy dpvo: ;
    rdfs:range dpvo:Policy ;
    rdfs:subPropertyOf dpvo:hasTechnicalOrganisationalMeasure ;
    sw:term_status "accepted"@en .

dpvo:hasProcessing a rdf:Property,
        owl:ObjectProperty ;
    rdfs:label "has processing"@en ;
    dct:created "2019-04-04"^^xsd:date ;
    dct:creator "Axel Polleres"^^xsd:string,
        "Bud Bruegger"^^xsd:string,
        "Harshvardhan J. Pandit"^^xsd:string,
        "Javier Fernández"^^xsd:string,
        "Mark Lizar"^^xsd:string ;
    dct:description "Indicates association with Processing"@en ;
    dct:modified "2020-11-04"^^xsd:date ;
    dct:source <https://specialprivacy.ercim.eu/> ;
    rdfs:domain owl:Thing ;
    rdfs:isDefinedBy dpvo: ;
    rdfs:range dpvo:Processing ;
    sw:term_status "accepted"@en .

dpvo:hasProcessingAutomation a rdf:Property,
        owl:ObjectProperty ;
    rdfs:label "has processing automation"@en ;
    dct:created "2022-08-13"^^xsd:date ;
    dct:creator "Harshvardhan J. Pandit"^^xsd:string ;
    dct:description "Indicates the use or extent of automation associated with processing"@en ;
    rdfs:domain owl:Thing ;
    rdfs:isDefinedBy dpvo: ;
    rdfs:range dpvo:AutomationOfProcessing ;
    sw:term_status "accepted"@en .

dpvo:hasProhibition a rdf:Property,
        owl:ObjectProperty ;
    rdfs:label "has prohibition"@en ;
    dct:created "2022-10-19"^^xsd:date ;
    dct:creator "Beatriz Esteves"^^xsd:string,
        "Georg P Krog"^^xsd:string,
        "Harshvardhan J. Pandit"^^xsd:string,
        "Paul Ryan"^^xsd:string ;
    dct:description "Specifying applicability or inclusion of a prohibition rule within specified context"@en ;
    rdfs:domain dpvo:Context ;
    rdfs:isDefinedBy dpvo: ;
    rdfs:range dpvo:Prohibition ;
    rdfs:subPropertyOf dpvo:hasRule ;
    sw:term_status "accepted"@en .

dpvo:hasPurpose a rdf:Property,
        owl:ObjectProperty ;
    rdfs:label "has purpose"@en ;
    dct:created "2019-04-04"^^xsd:date ;
    dct:creator "Axel Polleres"^^xsd:string,
        "Bud Bruegger"^^xsd:string,
        "Harshvardhan J. Pandit"^^xsd:string,
        "Javier Fernández"^^xsd:string,
        "Mark Lizar"^^xsd:string ;
    dct:description "Indicates association with Purpose"@en ;
    dct:modified "2020-11-04"^^xsd:date ;
    dct:source <https://specialprivacy.ercim.eu/> ;
    rdfs:domain owl:Thing ;
    rdfs:isDefinedBy dpvo: ;
    rdfs:range dpvo:Purpose ;
    sw:term_status "accepted"@en .

dpvo:hasRecipientDataController a rdf:Property,
        owl:ObjectProperty ;
    rdfs:label "has recipient data controller"@en ;
    dct:created "2022-02-09"^^xsd:date ;
    dct:creator "Georg P. Krog"^^xsd:string,
        "Harshvardhan J. Pandit"^^xsd:string,
        "Paul Ryan"^^xsd:string ;
    dct:description "Indiciates inclusion or applicability of a Data Controller as a Recipient of persona data"@en ;
    rdfs:domain owl:Thing ;
    rdfs:isDefinedBy dpvo: ;
    rdfs:range dpvo:DataController ;
    rdfs:subPropertyOf dpvo:hasRecipient ;
    sw:term_status "accepted"@en .

dpvo:hasRecipientThirdParty a rdf:Property,
        owl:ObjectProperty ;
    rdfs:label "has recipient third party"@en ;
    dct:created "2022-02-09"^^xsd:date ;
    dct:creator "Georg P. Krog"^^xsd:string,
        "Harshvardhan J. Pandit"^^xsd:string,
        "Paul Ryan"^^xsd:string ;
    dct:description "Indiciates inclusion or applicability of a Third Party as a Recipient of persona data"@en ;
    rdfs:domain owl:Thing ;
    rdfs:isDefinedBy dpvo: ;
    rdfs:range dpvo:ThirdParty ;
    rdfs:subPropertyOf dpvo:hasRecipient ;
    sw:term_status "accepted"@en .

dpvo:hasRelationWithDataSubject a rdf:Property,
        owl:ObjectProperty ;
    rdfs:label "has relation with data subject"@en ;
    dct:created "2022-06-21"^^xsd:date ;
    dct:creator "Georg P Krog"^^xsd:string,
        "Harshvardhan J. Pandit"^^xsd:string,
        "Julian Flake"^^xsd:string,
        "Paul Ryan"^^xsd:string ;
    dct:description "Indicates the relation between specified Entity and Data Subject"@en ;
    rdfs:domain dpvo:Entity ;
    rdfs:isDefinedBy dpvo: ;
    rdfs:range owl:Thing ;
    rdfs:subPropertyOf dpvo:hasEntity ;
    sw:term_status "accepted"@en .

dpvo:hasResidualRisk a rdf:Property,
        owl:ObjectProperty ;
    rdfs:label "has residual risk"@en ;
    dct:created "2022-07-20"^^xsd:date ;
    dct:creator "Georg P Krog"^^xsd:string,
        "Harshvardhan J. Pandit"^^xsd:string,
        "Julian Flake"^^xsd:string,
        "Paul Ryan"^^xsd:string ;
    dct:description "Indicates the associated risk is the remaining or residual risk from applying mitigation measures or treatments to this risk"@en ;
    rdfs:domain dpvo:Risk ;
    rdfs:isDefinedBy dpvo: ;
    rdfs:range dpvo:Risk ;
    sw:term_status "accepted"@en .

dpvo:hasResponsibleEntity a rdf:Property,
        owl:ObjectProperty ;
    rdfs:label "has responsible entity"@en ;
    dct:created "2022-03-02"^^xsd:date ;
    dct:creator "Harshvardhan J. Pandit"^^xsd:string ;
    dct:description "Specifies the indicated entity is responsible within some context"@en ;
    rdfs:domain owl:Thing ;
    rdfs:isDefinedBy dpvo: ;
    rdfs:range dpvo:Entity ;
    rdfs:subPropertyOf dpvo:hasEntity ;
    sw:term_status "accepted"@en .

dpvo:hasRight a rdf:Property,
        owl:ObjectProperty ;
    rdfs:label "has right"@en ;
    dct:created "2020-11-18"^^xsd:date ;
    dct:creator "Harshvardhan J. Pandit"^^xsd:string ;
    dct:description "Indicates use or applicability of Right"@en ;
    rdfs:domain owl:Thing ;
    rdfs:isDefinedBy dpvo: ;
    rdfs:range dpvo:Right ;
    sw:term_status "accepted"@en .

dpvo:hasRisk a rdf:Property,
        owl:ObjectProperty ;
    rdfs:label "has risk"@en ;
    dct:created "2020-11-18"^^xsd:date ;
    dct:creator "Harshvardhan J. Pandit"^^xsd:string ;
    dct:description "Indicates applicability of Risk"@en,
        "Indicates applicability of Risk for this concept"@en ;
    rdfs:domain owl:Thing ;
    rdfs:isDefinedBy dpvo: ;
    rdfs:range dpvo:Risk ;
    sw:term_status "accepted"@en .

dpvo:hasRiskLevel a rdf:Property,
        owl:ObjectProperty ;
    rdfs:label "has risk level"@en ;
    dct:created "2022-07-20"^^xsd:date ;
    dct:creator "Georg P Krog"^^xsd:string,
        "Harshvardhan J. Pandit"^^xsd:string,
        "Julian Flake"^^xsd:string,
        "Paul Ryan"^^xsd:string ;
    dct:description "Indicates the associated risk level associated with a risk"@en ;
    rdfs:domain dpvo:Risk ;
    rdfs:isDefinedBy dpvo: ;
    rdfs:range dpvo:RiskLevel ;
    sw:term_status "accepted"@en .

dpvo:hasScope a rdf:Property,
        owl:ObjectProperty ;
    rdfs:label "has scope"@en ;
    dct:created "2022-06-15"^^xsd:date ;
    dct:creator "Harshvardhan J. Pandit"^^xsd:string ;
    dct:description "Indicates the scope of specified concept or context"@en ;
    rdfs:domain owl:Thing ;
    rdfs:isDefinedBy dpvo: ;
    rdfs:range dpvo:Scope ;
    sw:term_status "accepted"@en .

dpvo:hasSector a rdf:Property,
        owl:ObjectProperty ;
    rdfs:label "has sector"@en ;
    dct:created "2019-04-05"^^xsd:date ;
    dct:description "Indicates the purpose is associated with activities in the indicated (Economic) Sector(s)"@en ;
    rdfs:domain owl:Thing ;
    rdfs:isDefinedBy dpvo: ;
    rdfs:range dpvo:Sector ;
    sw:term_status "accepted"@en .

dpvo:hasSeverity a rdf:Property,
        owl:ObjectProperty ;
    rdfs:label "has severity"@en ;
    dct:created "2022-07-20"^^xsd:date ;
    dct:creator "Georg P Krog"^^xsd:string,
        "Harshvardhan J. Pandit"^^xsd:string,
        "Julian Flake"^^xsd:string,
        "Paul Ryan"^^xsd:string ;
    dct:description "Indicates the severity associated with a concept"@en ;
    rdfs:domain owl:Thing ;
    rdfs:isDefinedBy dpvo: ;
    rdfs:range dpvo:Severity ;
    sw:term_status "accepted"@en .

dpvo:hasStorageCondition a rdf:Property,
        owl:ObjectProperty ;
    rdfs:label "has storage condition"@en ;
    dct:created "2022-08-13"^^xsd:date ;
    dct:creator "Axel Polleres"^^xsd:string,
        "Harshvardhan J. Pandit"^^xsd:string,
        "Mark Lizar"^^xsd:string,
        "Rob Brennan"^^xsd:string ;
    dct:description "Indicates information about storage condition"@en ;
    dct:source <https://specialprivacy.ercim.eu/> ;
    rdfs:domain owl:Thing ;
    rdfs:isDefinedBy dpvo: ;
    rdfs:range dpvo:StorageCondition ;
    sw:term_status "changed"@en .

dpvo:hasTechnicalMeasure a rdf:Property,
        owl:ObjectProperty ;
    rdfs:label "has technical measure"@en ;
    dct:created "2022-02-09"^^xsd:date ;
    dct:creator "Harshvardhan J. Pandit"^^xsd:string ;
    dct:description "Indicates use or applicability of Technical measure"@en ;
    rdfs:domain owl:Thing ;
    rdfs:isDefinedBy dpvo: ;
    rdfs:range dpvo:TechnicalMeasure ;
    rdfs:subPropertyOf dpvo:hasTechnicalOrganisationalMeasure ;
    sw:term_status "accepted"@en .

dpvo:hasThirdCountry a rdf:Property,
        owl:ObjectProperty ;
    rdfs:label "has third country"@en ;
    dct:created "2022-02-09"^^xsd:date ;
    dct:creator "Georg P Krog"^^xsd:string,
        "Harshvardhan J. Pandit"^^xsd:string ;
    dct:description "Indicates applicability or relevance of a 'third country'"@en ;
    rdfs:domain owl:Thing ;
    rdfs:isDefinedBy dpvo: ;
    rdfs:range dpvo:ThirdCountry ;
    rdfs:subPropertyOf dpvo:hasCountry ;
    sw:term_status "accepted"@en .

dpvo:isAfter a rdf:Property,
        owl:ObjectProperty ;
    rdfs:label "is after"@en ;
    dct:created "2022-03-02"^^xsd:date ;
    dct:creator "Georg P. Krog"^^xsd:string,
        "Harshvardhan J. Pandit"^^xsd:string,
        "Julian Flake"^^xsd:string ;
    dct:description "Indicates the specified concepts is 'after' this concept in some context"@en ;
    rdfs:domain owl:Thing ;
    rdfs:isDefinedBy dpvo: ;
    rdfs:range owl:Thing ;
    sw:term_status "accepted"@en .

dpvo:isAuthorityFor a rdf:Property,
        owl:ObjectProperty ;
    rdfs:label "is authority for"@en ;
    dct:created "2022-01-19"^^xsd:date ;
    dct:creator "Georg P Krog"^^xsd:string,
        "Harshvardhan J. Pandit"^^xsd:string ;
    dct:description "Indicates area, scope, or applicability of an Authority"@en ;
    rdfs:domain dpvo:Authority ;
    rdfs:isDefinedBy dpvo: ;
    rdfs:range owl:Thing ;
    sw:term_status "accepted"@en .

dpvo:isBefore a rdf:Property,
        owl:ObjectProperty ;
    rdfs:label "is before"@en ;
    dct:created "2022-03-02"^^xsd:date ;
    dct:creator "Georg P. Krog"^^xsd:string,
        "Harshvardhan J. Pandit"^^xsd:string,
        "Julian Flake"^^xsd:string ;
    dct:description "Indicates the specified concepts is 'before' this concept in some context"@en ;
    rdfs:domain owl:Thing ;
    rdfs:isDefinedBy dpvo: ;
    rdfs:range owl:Thing ;
    sw:term_status "accepted"@en .

dpvo:isExercisedAt a rdf:Property,
        owl:ObjectProperty ;
    rdfs:label "is exercised at"@en ;
    dct:created "2022-10-22"^^xsd:date ;
    dct:creator "Harshvardhan J. Pandit"^^xsd:string ;
    dct:description "Indicates context or information about exercising a right"@en ;
    rdfs:domain dpvo:ActiveRight ;
    rdfs:isDefinedBy dpvo: ;
    rdfs:range dpvo:RightExerciseNotice ;
    sw:term_status "accepted"@en .

dpvo:isImplementedByEntity a rdf:Property,
        owl:ObjectProperty ;
    rdfs:label "is implemented by entity"@en ;
    dct:created "2019-05-07"^^xsd:date ;
    dct:creator "Axel Polleres"^^xsd:string,
        "Beatriz Esteves"^^xsd:string,
        "Harshvardhan J. Pandit"^^xsd:string,
        "Julian Flake"^^xsd:string,
        "Paul Ryan"^^xsd:string ;
    dct:description "Indicates implementation details such as entities or agents"@en ;
    dct:modified "2022-01-26"^^xsd:date ;
    rdfs:comment "The use of 'entity' is inclusive of entities (e.g. Data Processor) as well as 'agent' (e.g. DPO). For indicating technological implementation, the property isImplementedByTechnology should be used."@en ;
    rdfs:domain owl:Thing ;
    rdfs:isDefinedBy dpvo: ;
    rdfs:range dpvo:Entity ;
    sw:term_status "changed"@en .

dpvo:isImplementedUsingTechnology a rdf:Property,
        owl:ObjectProperty ;
    rdfs:label "is implemented using technology"@en ;
    dct:created "2022-01-26"^^xsd:date ;
    dct:creator "Beatriz Esteves"^^xsd:string,
        "Harshvardhan J. Pandit"^^xsd:string,
        "Julian Flake"^^xsd:string,
        "Paul Ryan"^^xsd:string ;
    dct:description "Indicates implementation details such as technologies or processes"@en ;
    dct:modified "2022-06-15"^^xsd:date ;
    rdfs:comment "The term 'technology' is inclusive of technologies, processes, and methods."@en ;
    rdfs:domain owl:Thing ;
    rdfs:isDefinedBy dpvo: ;
    rdfs:range dpvo:Technology ;
    sw:term_status "changed"@en .

dpvo:isIndicatedAtTime a rdf:Property,
        owl:ObjectProperty ;
    rdfs:label "is indicated at time"@en ;
    dct:created "2022-06-21"^^xsd:date ;
    dct:creator "Georg P Krog"^^xsd:string,
        "Harshvardhan J. Pandit"^^xsd:string,
        "Julian Flake"^^xsd:string,
        "Paul Ryan"^^xsd:string ;
    dct:description "Specifies the temporal information for when the entity has indicated the specific context"@en ;
    rdfs:domain owl:Thing ;
    rdfs:isDefinedBy dpvo: ;
    sw:term_status "accepted"@en .

dpvo:isIndicatedBy a rdf:Property,
        owl:ObjectProperty ;
    rdfs:label "is indicated by"@en ;
    dct:created "2022-06-21"^^xsd:date ;
    dct:creator "Georg P Krog"^^xsd:string,
        "Harshvardhan J. Pandit"^^xsd:string,
        "Julian Flake"^^xsd:string,
        "Paul Ryan"^^xsd:string ;
    dct:description "Specifies entity who indicates the specific context"@en ;
    rdfs:domain owl:Thing ;
    rdfs:isDefinedBy dpvo: ;
    rdfs:range dpvo:Entity ;
    sw:term_status "accepted"@en .

dpvo:isMitigatedByMeasure a rdf:Property,
        owl:ObjectProperty ;
    rdfs:label "is mitigated by measure"@en ;
    dct:created "2022-02-09"^^xsd:date ;
    dct:creator "Harshvardhan J. Pandit"^^xsd:string ;
    dct:description "Indicate a risk is mitigated by specified measure"@en ;
    rdfs:domain dpvo:Risk ;
    rdfs:isDefinedBy dpvo: ;
    rdfs:range dpvo:RiskMitigationMeasure ;
    rdfs:subPropertyOf dpvo:hasTechnicalOrganisationalMeasure ;
    sw:term_status "accepted"@en .

dpvo:isPolicyFor a rdf:Property,
        owl:ObjectProperty ;
    rdfs:label "is policy for"@en ;
    dct:created "2022-01-26"^^xsd:date ;
    dct:creator "Harshvardhan J. Pandit"^^xsd:string ;
    dct:description "Indicates the context or application of policy"@en ;
    rdfs:domain dpvo:Policy ;
    rdfs:isDefinedBy dpvo: ;
    rdfs:range owl:Thing ;
    sw:term_status "accepted"@en .

dpvo:isRepresentativeFor a rdf:Property,
        owl:ObjectProperty ;
    rdfs:label "is representative for"@en ;
    dct:created "2022-11-09"^^xsd:date ;
    dct:creator "Harshvardhan J. Pandit"^^xsd:string ;
    dct:description "Indicates the entity is a representative for specified entity"@en ;
    rdfs:domain dpvo:Representative ;
    rdfs:isDefinedBy dpvo: ;
    rdfs:range dpvo:Entity ;
    rdfs:subPropertyOf dpvo:hasEntity ;
    sw:term_status "accepted"@en .

dpvo:isResidualRiskOf a rdf:Property,
        owl:ObjectProperty ;
    rdfs:label "is residual risk of"@en ;
    dct:created "2022-07-20"^^xsd:date ;
    dct:creator "Georg P Krog"^^xsd:string,
        "Harshvardhan J. Pandit"^^xsd:string,
        "Julian Flake"^^xsd:string,
        "Paul Ryan"^^xsd:string ;
    dct:description "Indicates this risk is the remaining or residual risk from applying mitigation measures or treatments to specified risk"@en ;
    rdfs:domain dpvo:Risk ;
    rdfs:isDefinedBy dpvo: ;
    rdfs:range dpvo:Risk ;
    sw:term_status "accepted"@en .

dpvo:mitigatesRisk a rdf:Property,
        owl:ObjectProperty ;
    rdfs:label "mitigates risk"@en ;
    dct:created "2020-11-04"^^xsd:date ;
    dct:creator "Harshvardhan J. Pandit"^^xsd:string ;
    dct:description "Indicates risks mitigated by this concept"@en ;
    rdfs:domain dpvo:RiskMitigationMeasure ;
    rdfs:isDefinedBy dpvo: ;
    rdfs:range dpvo:Risk ;
    sw:term_status "accepted"@en .

dpvo:ActiveRight a owl:Class ;
    rdfs:label "Active Right"@en ;
    dct:created "2022-10-22"^^xsd:date ;
    dct:creator "Beatriz Esteves"^^xsd:string,
        "Georg P Krog"^^xsd:string,
        "Harshvardhan J Pandit"^^xsd:string,
        "Paul Ryan"^^xsd:string ;
    dct:description "The right(s) applicable, provided, or expected that need to be (actively) exercised"@en ;
    rdfs:comment "Active rights require the entity to expressly exercise them. For example, a Data Subject exercising their right to withdraw their consent."@en ;
    rdfs:isDefinedBy dpvo: ;
    rdfs:subClassOf dpvo:Right ;
    sw:term_status "accepted"@en .

dpvo:Advertising a owl:Class ;
    rdfs:label "Advertising"@en ;
    dct:created "2020-11-04"^^xsd:date ;
    dct:creator "Beatriz Esteves"^^xsd:string,
        "Georg P Krog"^^xsd:string,
        "Harshvardhan J. Pandit"^^xsd:string ;
    dct:description "Purposes associated with conducting advertising i.e. process or artefact used to call attention to a product, service, etc. through announcements, notices, or other forms of communication"@en ;
    rdfs:comment "Advertising is a subset of Marketing. Advertising by itself does not indicate 'personalisation' i.e. personalised ads."@en ;
    rdfs:isDefinedBy dpvo: ;
    rdfs:subClassOf dpvo:Marketing ;
    sw:term_status "accepted"@en .

dpvo:AlgorithmicLogic a owl:Class ;
    rdfs:label "Algorithmic Logic"@en ;
    dct:created "2022-01-26"^^xsd:date ;
    dct:creator "Harshvardhan J. Pandit"^^xsd:string ;
    dct:description "The algorithmic logic applied or used"@en ;
    dct:modified "2022-06-15"^^xsd:date ;
    rdfs:comment "Algorithmic Logic is intended as a broad concept for explaining the use of algorithms and automated decisions making within Processing. To describe the actual algorithm, see the Algorithm concept."@en ;
    rdfs:isDefinedBy dpvo: ;
    rdfs:subClassOf dpvo:AutomationOfProcessing ;
    sw:term_status "accepted"@en .

dpvo:Alter a owl:Class ;
    rdfs:label "Alter"@en ;
    dct:created "2019-05-07"^^xsd:date ;
    dct:description "to change the data without changing it into something else"@en ;
    dct:source <https://eur-lex.europa.eu/eli/reg/2016/679/art_4/par_2/oj> ;
    rdfs:isDefinedBy dpvo: ;
    rdfs:subClassOf dpvo:Transform ;
    sw:term_status "accepted"@en .

dpvo:Applicant a owl:Class ;
    rdfs:label "Applicant"@en ;
    dct:created "2022-04-06"^^xsd:date ;
    dct:creator "Beatriz Esteves"^^xsd:string,
        "Georg P. Krog"^^xsd:string,
        "Harshvardhan J. Pandit"^^xsd:string,
        "Julian Flake"^^xsd:string,
        "Paul Ryan"^^xsd:string ;
    dct:description "Data subjects that are applicants in some context"@en ;
    rdfs:isDefinedBy dpvo: ;
    rdfs:subClassOf dpvo:DataSubject ;
    sw:term_status "accepted"@en .

dpvo:CollectedPersonalData a owl:Class ;
    rdfs:label "Collected Personal Data"@en ;
    dct:created "2022-03-30"^^xsd:date ;
    dct:creator "Harshvardhan J. Pandit"^^xsd:string ;
    dct:description "Personal Data that has been collected from another source such as the Data Subject"@en ;
    rdfs:comment "To indicate the source of data, use the DataSource concept with the hasDataSource relation"@en ;
    rdfs:isDefinedBy dpvo: ;
    rdfs:subClassOf dpvo:PersonalData ;
    sw:term_status "accepted"@en .

dpvo:CommunicationManagement a owl:Class ;
    rdfs:label "Communication Management"@en ;
    dct:created "2021-09-01"^^xsd:date ;
    dct:creator "David Hickey"^^xsd:string,
        "Georg P Krog"^^xsd:string,
        "Harshvardhan J. Pandit"^^xsd:string,
        "Paul Ryan"^^xsd:string ;
    dct:description "Communication Management refers to purposes associated with providing or managing communication activities e.g. to send an email for notifying some information"@en ;
    rdfs:comment "This purpose by itself does not sufficiently and clearly indicate what the communication is about. As such, it is recommended to combine it with another purpose to indicate the application. For example, Communication of Payment."@en ;
    rdfs:isDefinedBy dpvo: ;
    rdfs:subClassOf dpvo:Purpose ;
    sw:term_status "accepted"@en .

dpvo:ConsultationWithDataSubject a owl:Class ;
    rdfs:label "Consultation with Data Subject"@en ;
    dct:created "2022-06-15"^^xsd:date ;
    dct:creator "Georg P Krog"^^xsd:string,
        "Harshvardhan J. Pandit"^^xsd:string ;
    dct:description "Consultation with data subject(s) or their representative(s)"@en ;
    rdfs:isDefinedBy dpvo: ;
    rdfs:subClassOf dpvo:Consultation ;
    sw:term_status "accepted"@en .

dpvo:Customer a owl:Class ;
    rdfs:label "Customer"@en ;
    dct:created "2022-04-06"^^xsd:date ;
    dct:creator "Beatriz Esteves"^^xsd:string,
        "Georg P. Krog"^^xsd:string,
        "Harshvardhan J. Pandit"^^xsd:string,
        "Julian Flake"^^xsd:string,
        "Paul Ryan"^^xsd:string ;
    dct:description "Data subjects that purchase goods or services"@en ;
    rdfs:comment "note: for B2B relations where customers are organisations, this concept only applies for data subjects"@en ;
    rdfs:isDefinedBy dpvo: ;
    rdfs:subClassOf dpvo:DataSubject ;
    sw:term_status "accepted"@en .

dpvo:CustomerCare a owl:Class ;
    rdfs:label "Customer Care"@en ;
    dct:created "2019-04-05"^^xsd:date ;
    dct:creator "Axel Polleres"^^xsd:string,
        "Elmar Kiesling"^^xsd:string,
        "Fajar Ekaputra"^^xsd:string,
        "Harshvardhan J. Pandit"^^xsd:string,
        "Javier Fernandez"^^xsd:string,
        "Simon Steyskal"^^xsd:string ;
    dct:description "Customer Care refers to purposes associated with purposes for providing assistance, resolving issues, ensuring satisfaction, etc. in relation to services provided"@en ;
    rdfs:isDefinedBy dpvo: ;
    rdfs:seeAlso svpu:Feedback ;
    rdfs:subClassOf dpvo:CustomerManagement ;
    sw:term_status "accepted"@en .

dpvo:CustomerRelationshipManagement a owl:Class ;
    rdfs:label "Customer Relationship Management"@en ;
    dct:created "2021-09-08"^^xsd:date ;
    dct:creator "Beatriz"^^xsd:string,
        "Georg P Krog"^^xsd:string,
        "Harshvardhan J. Pandit"^^xsd:string ;
    dct:description "Customer Relationship Management refers to purposes associated with managing and analysing interactions with past, current, and potential customers"@en ;
    rdfs:isDefinedBy dpvo: ;
    rdfs:subClassOf dpvo:CustomerManagement ;
    sw:term_status "accepted"@en .

dpvo:CustomerSolvencyMonitoring a owl:Class ;
    rdfs:label "Customer Solvency Monitoring"@en ;
    dct:created "2021-09-08"^^xsd:date ;
    dct:creator "Beatriz"^^xsd:string,
        "Georg P Krog"^^xsd:string,
        "Harshvardhan J. Pandit"^^xsd:string ;
    dct:description "Customer Solvency Monitoring refers to purposes associated with monitor solvency of customers for financial diligence"@en ;
    dct:source <https://www.privacycommission.be/nl/model-voor-een-register-van-de-verwerkingsactiviteiten> ;
    rdfs:isDefinedBy dpvo: ;
    rdfs:subClassOf dpvo:CustomerManagement ;
    sw:term_status "accepted"@en .

dpvo:DataExporter a owl:Class ;
    rdfs:label "Data Exporter"@en ;
    dct:created "2021-09-08"^^xsd:date ;
    dct:creator "David Hickey"^^xsd:string,
        "Georg Krog"^^xsd:string,
        "Harshvardhan Pandit"^^xsd:string,
        "Paul Ryan"^^xsd:string ;
    dct:description "An entity that 'exports' data where exporting is considered a form of data transfer"@en ;
    dct:source <https://edpb.europa.eu/our-work-tools/our-documents/recommendations/recommendations-012020-measures-supplement-transfer_en> ;
    rdfs:comment "The EU, in particular the EDPB, uses data exporter the context of cross-border data transfers/flows. These concepts are not bound by jurisdictional or geopolitical scopes within DPV and can thus be used for any notion of exporting"@en ;
    rdfs:isDefinedBy dpvo: ;
    rdfs:subClassOf dpvo:LegalEntity ;
    sw:term_status "accepted"@en .

dpvo:DataImporter a owl:Class ;
    rdfs:label "Data Importer"@en ;
    dct:created "2021-09-08"^^xsd:date ;
    dct:creator "David Hickey"^^xsd:string,
        "Georg Krog"^^xsd:string,
        "Harshvardhan Pandit"^^xsd:string,
        "Paul Ryan"^^xsd:string ;
    dct:description "An entity that 'imports' data where importing is considered a form of data transfer"@en ;
    dct:source <https://edpb.europa.eu/our-work-tools/our-documents/recommendations/recommendations-012020-measures-supplement-transfer_en> ;
    rdfs:comment "The EU, in particular the EDPB, uses data importing the context of cross-border data transfers/flows. These concepts are not bound by jurisdictional or geopolitical scopes within DPV and can thus be used for any notion of importing"@en ;
    rdfs:isDefinedBy dpvo: ;
    rdfs:subClassOf dpvo:Recipient ;
    sw:term_status "accepted"@en .

dpvo:DataProtectionOfficer a owl:Class ;
    rdfs:label "Data Protection Officer"@en ;
    dct:created "2020-11-04"^^xsd:date ;
    dct:creator "Georg Krog"^^xsd:string,
        "Paul Ryan"^^xsd:string ;
    dct:description "An entity within or authorised by an organisation to monitor internal compliance, inform and advise on data protection obligations and act as a contact point for data subjects and the supervisory authority."@en ;
    dct:modified "2021-12-08"^^xsd:date ;
    dct:source <https://eur-lex.europa.eu/eli/reg/2016/679/art_37/oj> ;
    rdfs:isDefinedBy dpvo: ;
    rdfs:subClassOf dpvo:Representative ;
    sw:term_status "modified"@en .

dpvo:DecisionMaking a owl:Class ;
    rdfs:label "Decision Making"@en ;
    dct:created "2022-09-07"^^xsd:date ;
    dct:creator "Harshvardhan J. Pandit"^^xsd:string ;
    dct:description "Processing that involves decision making"@en ;
    rdfs:isDefinedBy dpvo: ;
    rdfs:subClassOf dpvo:ProcessingContext ;
    sw:term_status "accepted"@en .

dpvo:Derive a owl:Class ;
    rdfs:label "Derive"@en ;
    dct:created "2019-05-07"^^xsd:date ;
    dct:description "to create new derivative data from the original data"@en ;
    dct:source <https://specialprivacy.ercim.eu/vocabs/processing> ;
    rdfs:comment "Derive indicates data is present or obtainable from existing data. For data that is created without such existence, see Infer."@en ;
    rdfs:isDefinedBy dpvo: ;
    rdfs:seeAlso svpr:Derive ;
    rdfs:subClassOf dpvo:Obtain ;
    sw:term_status "accepted"@en .

dpvo:DerivedPersonalData a owl:Class ;
    rdfs:label "Derived Personal Data"@en ;
    dct:created "2019-05-07"^^xsd:date ;
    dct:creator "Elmar Kiesling; Harshvardhan J. Pandit"^^xsd:string,
        "Fajar Ekaputra"^^xsd:string ;
    dct:description "Personal Data that is obtained or derived from other data"@en ;
    dct:modified "2022-01-19"^^xsd:date ;
    dct:source <https://www.w3.org/community/dpvcg/> ;
    rdfs:comment "Derived Data is data that is obtained through processing of existing data, e.g. deriving first name from full name. To indicate data that is derived but which was not present or evident within the source data, InferredPersonalData should be used."@en ;
    rdfs:isDefinedBy dpvo: ;
    rdfs:seeAlso svd:Derived ;
    rdfs:subClassOf dpvo:PersonalData ;
    sw:term_status "accepted"@en .

dpvo:ExpressedConsent a owl:Class ;
    rdfs:label "Expressed Consent"@en ;
    dct:created "2022-06-21"^^xsd:date ;
    dct:creator "Georg P Krog"^^xsd:string,
        "Harshvardhan J. Pandit"^^xsd:string,
        "Julian Flake"^^xsd:string,
        "Paul Ryan"^^xsd:string ;
    dct:description "Consent that is expressed through an action intended to convey a consenting decision"@en ;
    rdfs:comment "Expressed consent requires the individual take a specific and unambigious action that directly indicates their consent. This action may be a part of other processes such as setting preferences, or agreeing to a contract, or other matters not relating to consent. An example of expressed consent is interacting with a checkbox within a dashboard or clicking a button on a web form"@en ;
    rdfs:isDefinedBy dpvo: ;
    rdfs:subClassOf dpvo:InformedConsent ;
    sw:term_status "accepted"@en .

dpvo:GeneratedPersonalData a owl:Class ;
    rdfs:label "Generated Personal Data"@en ;
    dct:created "2022-03-30"^^xsd:date ;
    dct:creator "Harshvardhan J. Pandit"^^xsd:string ;
    dct:description "Personal Data that is generated or brought into existence without relation to existing data i.e. it is not derived or inferred from other data"@en ;
    rdfs:comment "Generated Data is used to indicate data that is produced and is not derived or inferred from other data"@en ;
    rdfs:isDefinedBy dpvo: ;
    rdfs:subClassOf dpvo:PersonalData ;
    sw:term_status "accepted"@en .

dpvo:GovernmentalOrganisation a owl:Class ;
    rdfs:label "Governmental Organisation"@en ;
    dct:created "2022-02-02"^^xsd:date ;
    dct:creator "Harshvardhan J. Pandit"^^xsd:string ;
    dct:description "An organisation managed or part of government"@en ;
    dct:modified "2020-10-05"^^xsd:date ;
    rdfs:isDefinedBy dpvo: ;
    rdfs:subClassOf dpvo:Organisation ;
    sw:term_status "modified"@en .

dpvo:HumanInvolvementForInput a owl:NamedIndividual,
        dpvo:HumanInvolvement ;
    rdfs:label "Human Involvement for Input"@en ;
    dct:created "2022-09-07"^^xsd:date ;
    dct:creator "Harshvardhan J. Pandit"^^xsd:string ;
    dct:description "Human involvement for the purposes of providing inputs"@en ;
    rdfs:isDefinedBy dpvo: ;
    sw:term_status "accepted"@en .

dpvo:HumanInvolvementForOversight a owl:NamedIndividual,
        dpvo:HumanInvolvement ;
    rdfs:label "Human Involvement for Oversight"@en ;
    dct:created "2022-09-07"^^xsd:date ;
    dct:creator "Harshvardhan J. Pandit"^^xsd:string ;
    dct:description "Human involvement for the purposes of having oversight over a system, its operations, inputs, or outputs"@en ;
    rdfs:isDefinedBy dpvo: ;
    sw:term_status "accepted"@en .

dpvo:HumanInvolvementForVerification a owl:NamedIndividual,
        dpvo:HumanInvolvement ;
    rdfs:label "Human Involvement for Verification"@en ;
    dct:created "2022-09-07"^^xsd:date ;
    dct:creator "Harshvardhan J. Pandit"^^xsd:string ;
    dct:description "Human involvement for the purposes of verification of a system, its operations, inputs, or outputs"@en ;
    rdfs:isDefinedBy dpvo: ;
    sw:term_status "accepted"@en .

dpvo:HumanResourceManagement a owl:Class ;
    rdfs:label "Human Resource Management"@en ;
    dct:created "2021-09-01"^^xsd:date ;
    dct:creator "Beatriz Esteves"^^xsd:string,
        "David Hickey"^^xsd:string,
        "Georg P Krog"^^xsd:string,
        "Harshvardhan J. Pandit"^^xsd:string,
        "Paul Ryan"^^xsd:string ;
    dct:description "Purposes associated with managing humans and 'human resources' within the organisation for effective and efficient operations."@en ;
    dct:source <https://www.privacycommission.be/nl/model-voor-een-register-van-de-verwerkingsactiviteiten> ;
    rdfs:comment "HR is a broad concept. Its management includes, amongst others - recruiting employees and intermediaries e.g. brokers, independent representatives; payroll administration, remunerations, commissions, and wages; and application of social legislation."@en ;
    rdfs:isDefinedBy dpvo: ;
    rdfs:subClassOf dpvo:Purpose ;
    sw:term_status "accepted"@en .

dpvo:JointDataControllers a owl:Class ;
    rdfs:label "Joint Data Controllers"@en ;
    dct:created "2022-02-02"^^xsd:date ;
    dct:creator "Georg Krog"^^xsd:string,
        "Harshvardhan Pandit"^^xsd:string ;
    dct:description "A group of Data Controllers that jointly determine the purposes and means of processing"@en ;
    rdfs:comment "To indicate the membership, hasDataController may be used"@en ;
    rdfs:isDefinedBy dpvo: ;
    rdfs:subClassOf dpvo:DataController ;
    sw:term_status "accepted"@en .

dpvo:Justification a owl:Class ;
    rdfs:label "Justification"@en ;
    dct:created "2022-06-15"^^xsd:date ;
    dct:creator "Harshvardhan J. Pandit"^^xsd:string ;
    dct:description "A form of documentation providing reaosns, explanations, or justifications"@en ;
    rdfs:isDefinedBy dpvo: ;
    rdfs:subClassOf dpvo:Context ;
    sw:term_status "accepted"@en .

dpvo:Law a owl:Class ;
    rdfs:label "Law"@en ;
    dct:created "2022-01-19"^^xsd:date ;
    dct:creator "Harshvardhan J. Pandit"^^xsd:string ;
    dct:description "A law is a set of rules created by government or authorities"@en ;
    rdfs:isDefinedBy dpvo: ;
    sw:term_status "accepted"@en .

dpvo:Likelihood a owl:Class ;
    rdfs:label "Likelihood"@en ;
    dct:created "2022-07-22"^^xsd:date ;
    dct:creator "Harshvardhan J. Pandit"^^xsd:string ;
    dct:description "The likelihood or probability or chance of something taking place or occuring"@en ;
    rdfs:comment "Likelihood can be expressed in a subjective manner, such as 'Unlikely', or in a quantitative manner such as \"Twice in a Day\" (frequency per period). The suggestion is to use quantitative values, or to associate them with subjective terms used so as to enable accurate interpretations and interoperability. See the concepts related to Frequency and Duration for possible uses as a combination to express Likelihood."@en ;
    rdfs:isDefinedBy dpvo: ;
    sw:term_status "accepted"@en .

dpvo:NaturalPerson a owl:Class ;
    rdfs:label "Natural Person"@en ;
    dct:created "2022-02-09"^^xsd:date ;
    dct:creator "Harshvardhan J. Pandit"^^xsd:string ;
    dct:description "A human"@en ;
    rdfs:isDefinedBy dpvo: ;
    rdfs:subClassOf dpvo:Entity ;
    sw:term_status "accepted"@en .

dpvo:NonPersonalData a owl:Class ;
    rdfs:label "Non-Personal Data"@en ;
    dct:created "2022-01-19"^^xsd:date ;
    dct:creator "Harshvardhan J. Pandit"^^xsd:string ;
    dct:description "Data that is not Personal Data"@en ;
    rdfs:comment "The term NonPersonalData is provided to distinguish between PersonalData and other data, e.g. for indicating which data is regulated by privacy laws. To specify personal data that has been anonymised, the concept AnonymisedData should be used."@en ;
    rdfs:isDefinedBy dpvo: ;
    rdfs:subClassOf dpvo:Data ;
    sw:term_status "accepted"@en .

dpvo:Obligation a owl:Class ;
    rdfs:label "Obligation"@en ;
    dct:created "2022-10-19"^^xsd:date ;
    dct:creator "Beatriz Esteves"^^xsd:string,
        "Georg P Krog"^^xsd:string,
        "Harshvardhan J. Pandit"^^xsd:string,
        "Paul Ryan"^^xsd:string ;
    dct:description "A rule describing an obligation for performing an activity"@en ;
    rdfs:isDefinedBy dpvo: ;
    rdfs:subClassOf dpvo:Rule ;
    sw:term_status "accepted"@en .

dpvo:OptimisationForConsumer a owl:Class ;
    rdfs:label "Optimisation for Consumer"@en ;
    dct:created "2019-04-05"^^xsd:date ;
    dct:creator "Axel Polleres"^^xsd:string,
        "Elmar Kiesling"^^xsd:string,
        "Fajar Ekaputra"^^xsd:string,
        "Harshvardhan J. Pandit"^^xsd:string,
        "Javier Fernandez"^^xsd:string,
        "Simon Steyskal"^^xsd:string ;
    dct:description "Purposes associated with optimisation of activities and services for consumer or user"@en ;
    rdfs:comment "The term optmisation here refers to the efficiency of the service in terms of technical provision (or similar means) with benefits for everybody. Personalisation implies making changes that benefit the current user or persona."@en ;
    rdfs:isDefinedBy dpvo: ;
    rdfs:seeAlso svpu:Custom ;
    rdfs:subClassOf dpvo:ServiceOptimisation ;
    sw:term_status "accepted"@en .

dpvo:Organise a owl:Class ;
    rdfs:label "Organise"@en ;
    dct:created "2019-05-07"^^xsd:date ;
    dct:description "to organize data for arranging or classifying"@en ;
    dct:source <https://eur-lex.europa.eu/eli/reg/2016/679/art_4/par_2/oj> ;
    rdfs:isDefinedBy dpvo: ;
    rdfs:subClassOf dpvo:Processing ;
    sw:term_status "accepted"@en .

dpvo:Permission a owl:Class ;
    rdfs:label "Permission"@en ;
    dct:created "2022-10-19"^^xsd:date ;
    dct:creator "Beatriz Esteves"^^xsd:string,
        "Georg P Krog"^^xsd:string,
        "Harshvardhan J. Pandit"^^xsd:string,
        "Paul Ryan"^^xsd:string ;
    dct:description "A rule describing a permission to perform an activity"@en ;
    rdfs:isDefinedBy dpvo: ;
    rdfs:subClassOf dpvo:Rule ;
    sw:term_status "accepted"@en .

dpvo:PersonalDataHandling a owl:Class ;
    rdfs:label "Personal Data Handling"@en ;
    dct:created "2019-04-05"^^xsd:date ;
    dct:creator "Axel Polleres"^^xsd:string,
        "Javier Fernández"^^xsd:string ;
    dct:description "A high-level Class to describe 'data handling'. This can consist of personal data being processed for a purpose, involving entities, using technical and organisational measures, applicable risks, rights, and legal basis."@en ;
    dct:modified "2020-11-04"^^xsd:date ;
    rdfs:isDefinedBy dpvo: ;
    sw:term_status "accepted"@en .

dpvo:PersonalisedAdvertising a owl:Class ;
    rdfs:label "Personalised Advertising"@en ;
    dct:created "2020-11-04"^^xsd:date ;
    dct:creator "Beatriz Esteves"^^xsd:string,
        "Georg P Krog"^^xsd:string,
        "Harshvardhan J. Pandit"^^xsd:string ;
    dct:description "Purposes associated with creating and providing personalised advertising"@en ;
    rdfs:isDefinedBy dpvo: ;
    rdfs:subClassOf dpvo:Advertising,
        dpvo:Personalisation ;
    sw:term_status "accepted"@en .

dpvo:PrivacyNotice a owl:Class ;
    rdfs:label "Privacy Notice"@en ;
    dct:created "2021-09-08"^^xsd:date ;
    dct:creator "David Hickey"^^xsd:string,
        "Georg P Krog"^^xsd:string,
        "Harshvardhan J. Pandit"^^xsd:string,
        "Paul Ryan"^^xsd:string ;
    dct:description "Represents a notice or document outlining information regarding privacy"@en ;
    rdfs:isDefinedBy dpvo: ;
    rdfs:subClassOf dpvo:Notice ;
    sw:term_status "accepted"@en .

dpvo:Prohibition a owl:Class ;
    rdfs:label "Prohibition"@en ;
    dct:created "2022-10-19"^^xsd:date ;
    dct:creator "Beatriz Esteves"^^xsd:string,
        "Georg P Krog"^^xsd:string,
        "Harshvardhan J. Pandit"^^xsd:string,
        "Paul Ryan"^^xsd:string ;
    dct:description "A rule describing a prohibition to perform an activity"@en ;
    rdfs:isDefinedBy dpvo: ;
    rdfs:subClassOf dpvo:Rule ;
    sw:term_status "accepted"@en .

dpvo:Record a owl:Class ;
    rdfs:label "Record"@en ;
    dct:created "2019-05-07"^^xsd:date ;
    dct:description "to make a record (especially media)"@en ;
    dct:source <https://eur-lex.europa.eu/eli/reg/2016/679/art_4/par_2/oj> ;
    rdfs:isDefinedBy dpvo: ;
    rdfs:subClassOf dpvo:Obtain ;
    sw:term_status "accepted"@en .

dpvo:RecordsOfActivities a owl:Class ;
    rdfs:label "Records of Activities"@en ;
    dct:created "2021-09-08"^^xsd:date ;
    dct:creator "Georg P Krog"^^xsd:string,
        "Harshvardhan J. Pandit"^^xsd:string,
        "Paul Ryan"^^xsd:string ;
    dct:description "Records of activities within some context such as maintainence tasks or governance functions"@en ;
    rdfs:isDefinedBy dpvo: ;
    rdfs:subClassOf dpvo:OrganisationalMeasure ;
    sw:term_status "accepted"@en .

dpvo:RemoteLocation a owl:Class ;
    rdfs:label "Remote Location"@en ;
    dct:created "2022-06-15"^^xsd:date ;
    dct:creator "Harshvardhan J. Pandit"^^xsd:string ;
    dct:description "Location is remote i.e. not local"@en ;
    dct:modified "2020-10-05"^^xsd:date ;
    rdfs:isDefinedBy dpvo: ;
    rdfs:subClassOf dpvo:LocationLocality ;
    sw:term_status "modified"@en .

dpvo:RequestedServiceProvision a owl:Class ;
    rdfs:label "Requested Service Provision"@en ;
    dct:created "2021-09-08"^^xsd:date ;
    dct:creator "Beatriz Esteves"^^xsd:string,
        "Georg P Krog"^^xsd:string,
        "Harshvardhan J. Pandit"^^xsd:string ;
    dct:description "Purposes associated with delivering services as requested by user or consumer"@en ;
    rdfs:comment "The use of 'request' here includes where an user explicitly asks for the service and also when an established contract requires the provision of the service"@en ;
    rdfs:isDefinedBy dpvo: ;
    rdfs:subClassOf dpvo:ServiceProvision ;
    sw:term_status "accepted"@en .

dpvo:ReviewProcedure a owl:Class ;
    rdfs:label "Review Procedure"@en ;
    dct:created "2022-10-22"^^xsd:date ;
    dct:creator "Georg P Krog"^^xsd:string,
        "Harshvardhan J. Pandit"^^xsd:string ;
    dct:description "A procedure or process that reviews the correctness and validity of other measures and processes"@en ;
    rdfs:isDefinedBy dpvo: ;
    rdfs:subClassOf dpvo:OrganisationalMeasure ;
    sw:term_status "accepted"@en .

dpvo:RightExerciseNotice a owl:Class ;
    rdfs:label "Right Exercise Notice"@en ;
    dct:created "2022-10-22"^^xsd:date ;
    dct:creator "Beatriz Esteves"^^xsd:string,
        "Georg P Krog"^^xsd:string,
        "Harshvardhan J Pandit"^^xsd:string,
        "Paul Ryan"^^xsd:string ;
    dct:description "Information associated with exercising of an active right"@en ;
    rdfs:comment "This concept is intended for providing information regarding a right exercise. For specific instances of such exercises, see RightExerciseActivity and RightExerciseRecord."@en ;
    rdfs:isDefinedBy dpvo: ;
    sw:term_status "accepted"@en .

dpvo:RiskLevel a owl:Class ;
    rdfs:label "Risk Level"@en ;
    dct:created "2022-07-20"^^xsd:date ;
    dct:creator "Harshvardhan J. Pandit"^^xsd:string ;
    dct:description "The magnitude of a risk expressed as an indication to aid in its management"@en ;
    rdfs:comment "Risk Levels can be defined as a combination of different characteristics. For example, ISO 31073:2022 defines it as a combination of consequences and their likelihood. Another example would be the Risk Matrix where Risk Level is defined as a combination of Likelihood and Severity associated with the Risk."@en ;
    rdfs:isDefinedBy dpvo: ;
    sw:term_status "accepted"@en .

dpvo:Safeguard a owl:Class ;
    rdfs:label "Safeguard"@en ;
    dct:created "2021-09-22"^^xsd:date ;
    dct:creator "David Hickey"^^xsd:string,
        "Georg P Krog"^^xsd:string,
        "Harshvardhan J. Pandit"^^xsd:string,
        "Paul Ryan"^^xsd:string ;
    dct:description "A safeguard is a precautionary measure for the protection against or mitigation of negative effects"@en ;
    rdfs:comment "This concept is relevant given the requirement to assert safeguards in cross-border data transfers"@en ;
    rdfs:isDefinedBy dpvo: ;
    rdfs:subClassOf dpvo:OrganisationalMeasure ;
    sw:term_status "accepted"@en .

dpvo:Scope a owl:Class ;
    rdfs:label "Scope"@en ;
    dct:created "2022-06-15"^^xsd:date ;
    dct:creator "Harshvardhan J. Pandit"^^xsd:string ;
    dct:description "Indication of the extent or range or boundaries associated with(in) a context"@en ;
    rdfs:isDefinedBy dpvo: ;
    rdfs:subClassOf dpvo:Context ;
    sw:term_status "accepted"@en .

dpvo:Sector a owl:Class ;
    rdfs:label "Sector"@en ;
    dct:created "2019-04-05"^^xsd:date ;
    dct:creator "Axel Polleres"^^xsd:string,
        "Elmar Kiesling"^^xsd:string,
        "Fajar Ekaputra"^^xsd:string,
        "Harshvardhan J. Pandit"^^xsd:string,
        "Javier Fernandez"^^xsd:string,
        "Simon Steyskal"^^xsd:string ;
    dct:description "Sector describes the area of application or domain that indicates or restricts scope for interpretation and application of purpose e.g. Agriculture, Banking"@en ;
    rdfs:comment "There are various sector codes used commonly to indicate the domain of an organisation or business. Examples include NACE (EU), ISIC (UN), SIC and NAICS (USA)."@en ;
    rdfs:isDefinedBy dpvo: ;
    sw:term_status "accepted"@en .

dpvo:SecurityAssessment a owl:Class ;
    rdfs:label "Security Assessment"@en ;
    dct:created "2022-08-17"^^xsd:date ;
    dct:creator "Harshvardhan J. Pandit"^^xsd:string ;
    dct:description "Assessment of security intended to identity gaps, vulnerabilities, risks, and effectiveness of controls"@en ;
    dct:source <https://www.enisa.europa.eu/publications/5g-cybersecurity-standards> ;
    rdfs:isDefinedBy dpvo: ;
    rdfs:subClassOf dpvo:Assessment,
        dpvo:SecurityProcedure ;
    sw:term_status "accepted"@en .

dpvo:SensitivePersonalData a owl:Class ;
    rdfs:label "Sensitive Personal Data"@en ;
    dct:created "2022-01-19"^^xsd:date ;
    dct:creator "Harshvardhan J. Pandit"^^xsd:string ;
    dct:description "Personal data that is considered 'sensitive' in terms of privacy and/or impact, and therefore requires additional considerations and/or protection"@en ;
    rdfs:comment "Sensitivity' is a matter of context, and may be defined within legal frameworks. For GDPR, Special categories of personal data are considered a subset of sensitive data. To illustrate the difference between the two, consider the situation where Location data is collected, and which is considered 'sensitive' but not 'special'. As a probable rule, sensitive data require additional considerations whereas special category data requires additional legal basis / justifications."@en ;
    rdfs:isDefinedBy dpvo: ;
    rdfs:subClassOf dpvo:PersonalData ;
    sw:term_status "accepted"@en .

dpvo:Severity a owl:Class ;
    rdfs:label "Severity"@en ;
    dct:created "2022-07-21"^^xsd:date ;
    dct:creator "Harshvardhan J. Pandit"^^xsd:string ;
    dct:description "The magnitude of being unwanted or having negative effects such as harmful impacts"@en ;
    rdfs:comment "Severity can be associated with Risk, or its Consequences and Impacts"@en ;
    rdfs:isDefinedBy dpvo: ;
    sw:term_status "accepted"@en .

dpvo:Technology a owl:Class ;
    rdfs:label "Technology"@en ;
    dct:created "2022-01-26"^^xsd:date ;
    dct:creator "Harshvardhan J. Pandit"^^xsd:string ;
    dct:description "The technology, technological implementation, or any techniques, skills, methods, and processes used or applied"@en ;
    rdfs:comment "Examples (non-exhaustive) include: Algorithm, Process, Method, Skill, Database, Cookies, Server, Device"@en ;
    rdfs:isDefinedBy dpvo: ;
    sw:term_status "accepted"@en .

dpvo:ThirdCountry a owl:Class ;
    rdfs:label "Third Country"@en ;
    dct:created "2022-02-09"^^xsd:date ;
    dct:creator "Harshvardhan J. Pandit"^^xsd:string ;
    dct:description "Represents a country outside applicable or compatible jurisdiction as outlined in law"@en ;
    rdfs:isDefinedBy dpvo: ;
    rdfs:subClassOf dpvo:Country ;
    sw:term_status "accepted"@en .

dpvo:ThirdParty a owl:Class ;
    rdfs:label "Third Party"@en ;
    dct:created "2019-06-04"^^xsd:date ;
    dct:creator "Harshvardhan J. Pandit"^^xsd:string ;
    dct:description "A ‘third party’ means a natural or legal person, public authority, agency or body other than the data subject, controller, processor and people who, under the direct authority of the controller or processor, are authorised to process personal data."@en ;
    dct:source <https://eur-lex.europa.eu/eli/reg/2016/679/art_4/par_10/oj> ;
    rdfs:isDefinedBy dpvo: ;
    rdfs:subClassOf dpvo:Recipient ;
    sw:term_status "accepted"@en .

dpvo:Transfer a owl:Class ;
    rdfs:label "Transfer"@en ;
    dct:created "2019-05-07"^^xsd:date ;
    dct:description "to move data from one place to another"@en ;
    dct:source <https://specialprivacy.ercim.eu/vocabs/processing> ;
    rdfs:isDefinedBy dpvo: ;
    rdfs:seeAlso svpr:Transfer ;
    rdfs:subClassOf dpvo:Processing ;
    sw:term_status "accepted"@en .

dpvo:VitalInterest a owl:Class ;
    rdfs:label "Vital Interest"@en ;
    dct:created "2021-04-21"^^xsd:date ;
    dct:creator "Harshvardhan J. Pandit"^^xsd:string ;
    dct:description "Processing is necessary or required to protect vital interests of a data subject or other natural person"@en ;
    rdfs:isDefinedBy dpvo: ;
    rdfs:subClassOf dpvo:LegalBasis ;
    sw:term_status "accepted"@en .

dpvo:VitalInterestOfNaturalPerson a owl:Class ;
    rdfs:label "Vital Interest of Natural Person"@en ;
    dct:created "2021-04-21"^^xsd:date ;
    dct:creator "Georg P Krog"^^xsd:string,
        "Harshvardhan J. Pandit"^^xsd:string,
        "Paul Ryan"^^xsd:string ;
    dct:description "Processing is necessary or required to protect vital interests of a natural person"@en ;
    rdfs:isDefinedBy dpvo: ;
    rdfs:subClassOf dpvo:VitalInterest ;
    sw:term_status "accepted"@en .

dpvo:hasComplianceStatus a rdf:Property,
        owl:ObjectProperty ;
    rdfs:label "has compliance status"@en ;
    dct:created "2022-05-18"^^xsd:date ;
    dct:creator "Harshvardhan J. Pandit"^^xsd:string ;
    dct:description "Indicates the status of compliance of specified concept"@en ;
    rdfs:domain owl:Thing ;
    rdfs:isDefinedBy dpvo: ;
    rdfs:range dpvo:ComplianceStatus ;
    rdfs:subPropertyOf dpvo:hasStatus ;
    sw:term_status "accepted"@en .

dpvo:hasConsequence a rdf:Property,
        owl:ObjectProperty ;
    rdfs:label "has consequence"@en ;
    dct:created "2020-11-04"^^xsd:date ;
    dct:creator "Beatriz Esteves"^^xsd:string,
        "Fajar Ekaputra"^^xsd:string,
        "Georg P Krog"^^xsd:string,
        "Harshvardhan J. Pandit"^^xsd:string,
        "Julian Flake"^^xsd:string ;
    dct:description "Indicates consenquence(s) possible or arising from specified concept"@en ;
    dct:modified "2021-09-21"^^xsd:date ;
    rdfs:comment "Removed plural suffix for consistency"@en ;
    rdfs:domain owl:Thing ;
    rdfs:isDefinedBy dpvo: ;
    rdfs:range dpvo:Consequence ;
    sw:term_status "accepted"@en .

dpvo:hasConsequenceOn a rdf:Property,
        owl:ObjectProperty ;
    rdfs:label "has consequence on"@en ;
    dct:created "2022-11-24"^^xsd:date ;
    dct:creator "Georg P Krog"^^xsd:string,
        "Harshvardhan J. Pandit"^^xsd:string ;
    dct:description "Indicates the thing (e.g. plan, process, or entity) affected by a consequence"@en ;
    rdfs:domain dpvo:Consequence ;
    rdfs:isDefinedBy dpvo: ;
    rdfs:range owl:Thing ;
    sw:term_status "accepted"@en .

dpvo:hasCountry a rdf:Property,
        owl:ObjectProperty ;
    rdfs:label "has country"@en ;
    dct:created "2022-01-19"^^xsd:date ;
    dct:creator "Georg P Krog"^^xsd:string,
        "Harshvardhan J. Pandit"^^xsd:string ;
    dct:description "Indicates applicability of specified country"@en ;
    rdfs:domain owl:Thing ;
    rdfs:isDefinedBy dpvo: ;
    rdfs:range dpvo:Country ;
    rdfs:subPropertyOf dpvo:hasLocation ;
    sw:term_status "accepted"@en .

dpvo:hasData a rdf:Property,
        owl:ObjectProperty ;
    rdfs:label "has data"@en ;
    dct:created "2022-08-18"^^xsd:date ;
    dct:creator "Harshvardhan J. Pandit"^^xsd:string ;
    dct:description "Indicates associated with Data (may or may not be personal)"@en ;
    rdfs:domain owl:Thing ;
    rdfs:isDefinedBy dpvo: ;
    rdfs:range dpvo:Data ;
    sw:term_status "accepted"@en .

dpvo:hasDataController a rdf:Property,
        owl:ObjectProperty ;
    rdfs:label "has data controller"@en ;
    dct:created "2019-04-04"^^xsd:date ;
    dct:creator "Axel Polleres"^^xsd:string,
        "Bud Bruegger"^^xsd:string,
        "Harshvardhan J. Pandit"^^xsd:string,
        "Javier Fernández"^^xsd:string,
        "Mark Lizar"^^xsd:string ;
    dct:description "Indicates association with Data Controller"@en ;
    dct:modified "2020-11-04"^^xsd:date ;
    rdfs:domain owl:Thing ;
    rdfs:isDefinedBy dpvo: ;
    rdfs:range dpvo:DataController,
        dpvo:LegalEntity ;
    rdfs:subPropertyOf dpvo:hasEntity ;
    sw:term_status "accepted"@en .

dpvo:hasLocation a rdf:Property,
        owl:ObjectProperty ;
    rdfs:label "has location"@en ;
    dct:created "2019-04-05"^^xsd:date ;
    dct:creator "Axel Polleres"^^xsd:string,
        "Harshvardhan J. Pandit"^^xsd:string,
        "Mark Lizar"^^xsd:string,
        "Rob Brennan"^^xsd:string ;
    dct:description "Indicates information about location"@en ;
    dct:source <https://specialprivacy.ercim.eu/> ;
    rdfs:domain owl:Thing ;
    rdfs:isDefinedBy dpvo: ;
    rdfs:range dpvo:Location ;
    sw:term_status "accepted"@en .

dpvo:hasOrganisationalMeasure a rdf:Property,
        owl:ObjectProperty ;
    rdfs:label "has organisational measure"@en ;
    dct:created "2022-02-09"^^xsd:date ;
    dct:creator "Harshvardhan J. Pandit"^^xsd:string ;
    dct:description "Indicates use or applicability of Organisational measure"@en ;
    rdfs:domain owl:Thing ;
    rdfs:isDefinedBy dpvo: ;
    rdfs:range dpvo:OrganisationalMeasure ;
    rdfs:subPropertyOf dpvo:hasTechnicalOrganisationalMeasure ;
    sw:term_status "accepted"@en .

dpvo:hasRepresentative a rdf:Property,
        owl:ObjectProperty ;
    rdfs:label "has representative"@en ;
    dct:created "2020-11-04"^^xsd:date ;
    dct:creator "Beatriz Esteves"^^xsd:string,
        "Georg P Krog"^^xsd:string,
        "Harshvardhan J.Pandit"^^xsd:string,
        "Paul Ryan"^^xsd:string ;
    dct:description "Specifies representative of the legal entity"@en ;
    rdfs:domain dpvo:Entity ;
    rdfs:isDefinedBy dpvo: ;
    rdfs:range dpvo:Representative ;
    rdfs:subPropertyOf dpvo:hasEntity ;
    sw:term_status "accepted"@en .

dpvo:AccessControlMethod a owl:Class ;
    rdfs:label "Access Control Method"@en ;
    dct:created "2019-04-05"^^xsd:date ;
    dct:creator "Axel Polleres"^^xsd:string,
        "Harshvardhan J. Pandit"^^xsd:string,
        "Mark Lizar"^^xsd:string,
        "Rob Brennan"^^xsd:string ;
    dct:description "Methods which restrict access to a place or resource"@en ;
    rdfs:isDefinedBy dpvo: ;
    rdfs:subClassOf dpvo:TechnicalMeasure ;
    sw:term_status "accepted"@en .

dpvo:AuthorisationProcedure a owl:Class ;
    rdfs:label "Authorisation Procedure"@en ;
    dct:created "2019-04-05"^^xsd:date ;
    dct:creator "Axel Polleres"^^xsd:string,
        "Harshvardhan J. Pandit"^^xsd:string,
        "Mark Lizar"^^xsd:string,
        "Rob Brennan"^^xsd:string ;
    dct:description "Procedures for determining authorisation through permission or authority"@en ;
    rdfs:comment "non-technical authorisation procedures: How is it described on an organisational level, who gets access to the data"@en ;
    rdfs:isDefinedBy dpvo: ;
    rdfs:subClassOf dpvo:OrganisationalMeasure ;
    sw:term_status "accepted"@en .

dpvo:CertificationSeal a owl:Class ;
    rdfs:label "Certification and Seal"@en ;
    dct:created "2019-04-05"^^xsd:date ;
    dct:creator "Axel Polleres"^^xsd:string,
        "Harshvardhan J. Pandit"^^xsd:string,
        "Mark Lizar"^^xsd:string,
        "Rob Brennan"^^xsd:string ;
    dct:description "Certifications, seals, and marks indicating compliance to regulations or practices"@en ;
    rdfs:isDefinedBy dpvo: ;
    rdfs:subClassOf dpvo:OrganisationalMeasure ;
    sw:term_status "accepted"@en .

dpvo:ConformanceStatus a owl:Class ;
    rdfs:label "Conformance Status"@en ;
    dct:created "2022-10-22"^^xsd:date ;
    dct:creator "Harshvardhan J. Pandit"^^xsd:string ;
    dct:description "Status associated with conformance to a standard, guideline, code, or recommendation"@en ;
    rdfs:isDefinedBy dpvo: ;
    rdfs:subClassOf dpvo:Status ;
    sw:term_status "accepted"@en .

dpvo:Consent a owl:Class ;
    rdfs:label "Consent"@en ;
    dct:created "2021-04-07"^^xsd:date ;
    dct:creator "Harshvardhan J. Pandit"^^xsd:string ;
    dct:description "Consent of the Data Subject for specified processing"@en ;
    rdfs:isDefinedBy dpvo: ;
    rdfs:subClassOf dpvo:LegalBasis ;
    sw:term_status "accepted"@en .

dpvo:ConsentStatusValidForProcessing a owl:Class ;
    rdfs:label "Consent Status Valid for Processing"@en ;
    dct:created "2022-06-22"^^xsd:date ;
    dct:creator "Georg P Krog"^^xsd:string,
        "Harshvardhan J. Pandit"^^xsd:string,
        "Julian Flake"^^xsd:string,
        "Paul Ryan"^^xsd:string ;
    dct:description "States of consent that can be used as valid justifications for processing data"@en ;
    dct:source <https://w3id.org/GConsent> ;
    rdfs:comment "Practically, given consent is the only valid state for processing"@en ;
    rdfs:isDefinedBy dpvo: ;
    rdfs:subClassOf dpvo:ConsentStatus ;
    sw:term_status "accepted"@en .

dpvo:Consult a owl:Class ;
    rdfs:label "Consult"@en ;
    dct:created "2019-05-07"^^xsd:date ;
    dct:description "to consult or query data"@en ;
    dct:source <https://eur-lex.europa.eu/eli/reg/2016/679/art_4/par_2/oj>,
        <https://specialprivacy.ercim.eu/vocabs/processing> ;
    rdfs:isDefinedBy dpvo: ;
    rdfs:seeAlso svpr:Query ;
    rdfs:subClassOf dpvo:Use ;
    sw:term_status "accepted"@en .

dpvo:Contract a owl:Class ;
    rdfs:label "Contract"@en ;
    dct:created "2021-04-07"^^xsd:date ;
    dct:creator "Harshvardhan J. Pandit"^^xsd:string ;
    dct:description "Creation, completion, fulfilment, or performance of a contract involving specified processing"@en ;
    rdfs:isDefinedBy dpvo: ;
    rdfs:subClassOf dpvo:LegalAgreement,
        dpvo:LegalBasis ;
    sw:term_status "accepted"@en .

dpvo:Country a owl:Class ;
    rdfs:label "Country"@en ;
    dct:created "2022-01-19"^^xsd:date ;
    dct:creator "Georg P Krog"^^xsd:string,
        "Harshvardhan J. Pandit"^^xsd:string ;
    dct:description "A political entity indicative of a sovereign or non-sovereign territorial state comprising of distinct geographical areas"@en ;
    rdfs:comment "The definition of country is not intended for political interpretation. DPVCG welcomes alternate definitions based in existing sources with global scope, such as UN or ISO."@en ;
    rdfs:isDefinedBy dpvo: ;
    rdfs:subClassOf dpvo:Location ;
    sw:term_status "accepted"@en .

dpvo:CreditChecking a owl:Class ;
    rdfs:label "Credit Checking"@en ;
    dct:created "2022-04-20"^^xsd:date ;
    dct:creator "Harshvardhan J. Pandit"^^xsd:string ;
    dct:description "Purposes associated with monitoring, performing, or assessing credit worthiness or solvency"@en ;
    rdfs:isDefinedBy dpvo: ;
    rdfs:subClassOf dpvo:CustomerSolvencyMonitoring ;
    sw:term_status "accepted"@en .

dpvo:DataProcessingRecord a owl:Class ;
    rdfs:label "Data Processing Record"@en ;
    dct:created "2021-09-08"^^xsd:date ;
    dct:creator "Harshvardhan J. Pandit"^^xsd:string ;
    dct:description "Record of personal data processing, whether ex-ante or ex-post"@en ;
    rdfs:isDefinedBy dpvo: ;
    rdfs:subClassOf dpvo:RecordsOfActivities ;
    sw:term_status "accepted"@en .

dpvo:DataProcessor a owl:Class ;
    rdfs:label "Data Processor"@en ;
    dct:created "2019-06-04"^^xsd:date ;
    dct:creator "Harshvardhan J. Pandit"^^xsd:string ;
    dct:description "A ‘processor’ means a natural or legal person, public authority, agency or other body which processes personal data on behalf of the controller."@en ;
    dct:source <https://eur-lex.europa.eu/eli/reg/2016/679/art_4/par_8/oj> ;
    rdfs:isDefinedBy dpvo: ;
    rdfs:subClassOf dpvo:Recipient ;
    sw:term_status "accepted"@en .

dpvo:DataSanitisationTechnique a owl:Class ;
    rdfs:label "Data Sanitisation Technique"@en ;
    dct:created "2022-08-17"^^xsd:date ;
    dct:creator "Harshvardhan J. Pandit"^^xsd:string ;
    dct:description "Cleaning or any removal or re-organisation of elements in data based on selective criteria"@en ;
    dct:source <https://www.enisa.europa.eu/publications/reference-incident-classification-taxonomy/> ;
    rdfs:isDefinedBy dpvo: ;
    rdfs:subClassOf dpvo:TechnicalMeasure ;
    sw:term_status "accepted"@en .

dpvo:Deidentification a owl:Class ;
    rdfs:label "De-Identification"@en ;
    dct:created "2019-04-05"^^xsd:date ;
    dct:creator "Axel Polleres"^^xsd:string,
        "Harshvardhan J. Pandit"^^xsd:string,
        "Mark Lizar"^^xsd:string,
        "Rob Brennan"^^xsd:string ;
    dct:description "Removal of identity or information to reduce identifiability"@en ;
    dct:modified "2022-11-24"^^xsd:date ;
    dct:source <https://nvlpubs.nist.gov/nistpubs/ir/2015/NIST.IR.8053.pdf> ;
    rdfs:isDefinedBy dpvo: ;
    rdfs:subClassOf dpvo:DataSanitisationTechnique ;
    sw:term_status "modified"@en .

dpvo:EvaluationScoring a owl:Class ;
    rdfs:label "Evaluation and Scoring"@en ;
    dct:created "2020-11-04"^^xsd:date ;
    dct:creator "Harshvardhan J. Pandit"^^xsd:string,
        "Piero Bonatti"^^xsd:string ;
    dct:description "Processing that involves evaluation and scoring of individuals"@en ;
    dct:source <https://eur-lex.europa.eu/eli/reg/2016/679/art_4/par_2/oj> ;
    rdfs:isDefinedBy dpvo: ;
    rdfs:subClassOf dpvo:ProcessingContext ;
    sw:term_status "accepted"@en .

dpvo:FixedLocation a owl:Class ;
    rdfs:label "Fixed Location"@en ;
    dct:created "2022-06-15"^^xsd:date ;
    dct:creator "Harshvardhan J. Pandit"^^xsd:string ;
    dct:description "Location that is fixed i.e. known to occur at a specific place"@en ;
    dct:modified "2020-10-05"^^xsd:date ;
    rdfs:isDefinedBy dpvo: ;
    rdfs:subClassOf dpvo:LocationFixture ;
    sw:term_status "modified"@en .

dpvo:FraudPreventionAndDetection a owl:Class ;
    rdfs:label "Fraud Prevention and Detection"@en ;
    dct:created "2019-04-05"^^xsd:date ;
    dct:creator "Axel Polleres"^^xsd:string,
        "Elmar Kiesling"^^xsd:string,
        "Fajar Ekaputra"^^xsd:string,
        "Harshvardhan J. Pandit"^^xsd:string,
        "Javier Fernandez"^^xsd:string,
        "Simon Steyskal"^^xsd:string ;
    dct:description "Purposes associated with fraud detection, prevention, and mitigation"@en ;
    rdfs:isDefinedBy dpvo: ;
    rdfs:seeAlso svpu:Government ;
    rdfs:subClassOf dpvo:EnforceSecurity ;
    sw:term_status "accepted"@en .

dpvo:FulfilmentOfObligation a owl:Class ;
    rdfs:label "Fulfilment of Obligation"@en ;
    dct:created "2022-11-09"^^xsd:date ;
    dct:creator "Georg P Krog"^^xsd:string,
        "Harshvardhan J. Pandit"^^xsd:string ;
    dct:description "Purposes associated with carrying out data processing to fulfill an obligation"@en ;
    rdfs:isDefinedBy dpvo: ;
    rdfs:subClassOf dpvo:Purpose ;
    sw:term_status "accepted"@en .

dpvo:Importance a owl:Class ;
    rdfs:label "Importance"@en ;
    dct:created "2022-02-09"^^xsd:date ;
    dct:creator "Beatriz Esteves"^^xsd:string,
        "Georg P Krog"^^xsd:string,
        "Harshvardhan J. Pandit"^^xsd:string,
        "Julian Flake"^^xsd:string,
        "Paul Ryan"^^xsd:string ;
    dct:description "An indication of 'importance' within a context"@en ;
    rdfs:comment "Importance can be used to express importance, desirability, relevance, or significance as a context."@en ;
    rdfs:isDefinedBy dpvo: ;
    rdfs:subClassOf dpvo:Context ;
    sw:term_status "accepted"@en .

dpvo:InformedConsent a owl:Class ;
    rdfs:label "Informed Consent"@en ;
    dct:created "2022-06-21"^^xsd:date ;
    dct:creator "Georg P Krog"^^xsd:string,
        "Harshvardhan J. Pandit"^^xsd:string,
        "Julian Flake"^^xsd:string,
        "Paul Ryan"^^xsd:string ;
    dct:description "Consent that is informed i.e. with the requirement to provide sufficient information to make a consenting decision"@en ;
    rdfs:comment "The specifics for what information should be provided or made available will depend on the context, use-case, or relevant legal requirements"@en ;
    rdfs:isDefinedBy dpvo: ;
    rdfs:subClassOf dpvo:Consent ;
    sw:term_status "accepted"@en .

dpvo:LocationLocality a owl:Class ;
    rdfs:label "Location Locality"@en ;
    dct:created "2022-06-15"^^xsd:date ;
    dct:creator "Harshvardhan J. Pandit"^^xsd:string ;
    dct:description "Locality refers to whether the specified location is local within some context, e.g. for the user"@en ;
    dct:modified "2022-10-04"^^xsd:date ;
    rdfs:isDefinedBy dpvo: ;
    rdfs:subClassOf dpvo:Location ;
    sw:term_status "modified"@en .

dpvo:Personalisation a owl:Class ;
    rdfs:label "Personalisation"@en ;
    dct:created "2021-09-01"^^xsd:date ;
    dct:creator "Harshvardhan J. Pandit"^^xsd:string ;
    dct:description "Purposes associated with creating and providing customisation based on attributes and/or needs of person(s) or context(s)."@en ;
    rdfs:comment "This term is a blanket purpose category for indicating personalisation of some other purpose, e.g. by creating a subclass of the other concept and Personalisation"@en ;
    rdfs:isDefinedBy dpvo: ;
    rdfs:subClassOf dpvo:Purpose ;
    sw:term_status "accepted"@en .

dpvo:PersonnelManagement a owl:Class ;
    rdfs:label "Personnel Management"@en ;
    dct:created "2022-03-30"^^xsd:date ;
    dct:creator "Harshvardhan J. Pandit"^^xsd:string,
        "Paul Ryan"^^xsd:string ;
    dct:description "Purposes associated with management of personnel associated with the organisation e.g. evaluation and management of employees and intermediaries"@en ;
    dct:source <https://www.privacycommission.be/nl/model-voor-een-register-van-de-verwerkingsactiviteiten> ;
    rdfs:isDefinedBy dpvo: ;
    rdfs:subClassOf dpvo:HumanResourceManagement ;
    sw:term_status "accepted"@en .

dpvo:ProvidePersonalisedRecommendations a owl:Class ;
    rdfs:label "Provide Personalised Recommendations"@en ;
    dct:created "2019-11-26"^^xsd:date ;
    dct:creator "Harshvardhan J. Pandit"^^xsd:string,
        "Rudy Jacob"^^xsd:string ;
    dct:description "Purposes associated with creating and providing personalised recommendations"@en ;
    dct:modified "2022-10-14"^^xsd:date ;
    dct:source <https://specialprivacy.ercim.eu/> ;
    rdfs:isDefinedBy dpvo: ;
    rdfs:subClassOf dpvo:ServicePersonalisation ;
    sw:term_status "accepted"@en .

dpvo:Remove a owl:Class ;
    rdfs:label "Remove"@en ;
    dct:created "2019-05-07"^^xsd:date ;
    dct:description "to destruct or erase data"@en ;
    dct:source <https://eur-lex.europa.eu/eli/reg/2016/679/art_4/par_2/oj> ;
    rdfs:isDefinedBy dpvo: ;
    rdfs:subClassOf dpvo:Processing ;
    sw:term_status "accepted"@en .

dpvo:RiskMitigationMeasure a owl:Class ;
    rdfs:label "Risk Mitigation Measure"@en ;
    dct:created "2020-11-04"^^xsd:date ;
    dct:creator "Georg P Krog"^^xsd:string,
        "Harshvardhan J. Pandit"^^xsd:string,
        "Paul Ryan"^^xsd:string ;
    dct:description "Measures intended to mitigate, minimise, or prevent risk."@en ;
    rdfs:isDefinedBy dpvo: ;
    rdfs:subClassOf dpvo:TechnicalOrganisationalMeasure ;
    sw:term_status "accepted"@en .

dpvo:ServiceOptimisation a owl:Class ;
    rdfs:label "Service Optimisation"@en ;
    dct:created "2019-04-05"^^xsd:date ;
    dct:creator "Axel Polleres"^^xsd:string,
        "Elmar Kiesling"^^xsd:string,
        "Fajar Ekaputra"^^xsd:string,
        "Harshvardhan J. Pandit"^^xsd:string,
        "Javier Fernandez"^^xsd:string,
        "Simon Steyskal"^^xsd:string ;
    dct:description "Purposes associated with optimisation of services or activities"@en ;
    rdfs:comment "Subclass of ServiceProvision since optimisation is usually considered part of providing services"@en ;
    rdfs:isDefinedBy dpvo: ;
    rdfs:subClassOf dpvo:ServiceProvision ;
    sw:term_status "accepted"@en .

dpvo:ConsentStatus a owl:Class ;
    rdfs:label "Consent Status"@en ;
    dct:created "2022-06-22"^^xsd:date ;
    dct:creator "Georg P Krog"^^xsd:string,
        "Harshvardhan J. Pandit"^^xsd:string,
        "Julian Flake"^^xsd:string,
        "Paul Ryan"^^xsd:string ;
    dct:description "The state or status of 'consent' that provides information reflecting its operational status and validity for processing data"@en ;
    dct:source <https://w3id.org/GConsent> ;
    rdfs:comment "States are useful as information artefacts to implement them in controlling processing, and to reflect the process and flow of obtaining and maintaining consent. For example, a database table that stores consent states for specific processing and can be queried to obtain them in an efficient manner. States are also useful in investigations to determine the use and validity of consenting practices"@en ;
    rdfs:isDefinedBy dpvo: ;
    rdfs:subClassOf dpvo:Status ;
    sw:term_status "accepted"@en .

dpvo:Consultation a owl:Class ;
    rdfs:label "Consultation"@en ;
    dct:created "2020-11-04"^^xsd:date ;
    dct:creator "Georg P Krog"^^xsd:string,
        "Harshvardhan J. Pandit"^^xsd:string,
        "Paul Ryan"^^xsd:string ;
    dct:description "Consultation is a process of receiving feedback, advice, or opinion from an external agency"@en ;
    rdfs:isDefinedBy dpvo: ;
    rdfs:subClassOf dpvo:OrganisationalMeasure ;
    sw:term_status "accepted"@en .

dpvo:Damage a owl:Class ;
    rdfs:label "Damage"@en ;
    dct:created "2022-03-30"^^xsd:date ;
    dct:creator "Harshvardhan J. Pandit"^^xsd:string ;
    dct:description "Impact that acts as or causes damages"@en ;
    rdfs:isDefinedBy dpvo: ;
    rdfs:subClassOf dpvo:Impact ;
    sw:term_status "accepted"@en .

dpvo:DataController a owl:Class ;
    rdfs:label "Data Controller"@en ;
    dct:created "2019-04-05"^^xsd:date ;
    dct:creator "Axel Polleres"^^xsd:string,
        "Javier Fernández"^^xsd:string ;
    dct:description "The individual or organisation that decides (or controls) the purpose(s) of processing personal data."@en ;
    dct:modified "2020-11-04"^^xsd:date ;
    dct:source <https://eur-lex.europa.eu/eli/reg/2016/679/art_4/par_7/oj> ;
    rdfs:comment "The terms 'Controller' is usually the more common form of indicating a Data Controller. In ISO/IEC the term 'PII Controller' is used."@en ;
    rdfs:isDefinedBy dpvo: ;
    rdfs:subClassOf dpvo:LegalEntity ;
    sw:term_status "accepted"@en .

dpvo:GuidelinesPrinciple a owl:Class ;
    rdfs:label "GuidelinesPrinciple"@en ;
    dct:created "2019-04-05"^^xsd:date ;
    dct:creator "Axel Polleres"^^xsd:string,
        "Harshvardhan J. Pandit"^^xsd:string,
        "Mark Lizar"^^xsd:string,
        "Rob Brennan"^^xsd:string ;
    dct:description "Guidelines or Principles regarding processing and operational measures"@en ;
    rdfs:isDefinedBy dpvo: ;
    rdfs:subClassOf dpvo:OrganisationalMeasure ;
    sw:term_status "accepted"@en .

dpvo:LegitimateInterest a owl:Class ;
    rdfs:label "Legitimate Interest"@en ;
    dct:created "2021-05-19"^^xsd:date ;
    dct:creator "Harshvardhan J. Pandit"^^xsd:string ;
    dct:description "Legitimate Interests of a Party as justification for specified processing"@en ;
    rdfs:isDefinedBy dpvo: ;
    rdfs:subClassOf dpvo:LegalBasis ;
    sw:term_status "accepted"@en .

dpvo:Necessity a owl:Class ;
    rdfs:label "Necessity"@en ;
    dct:created "2022-02-12"^^xsd:date ;
    dct:creator "Beatriz Esteves"^^xsd:string,
        "Georg P Krog"^^xsd:string,
        "Harshvardhan J. Pandit"^^xsd:string,
        "Julian Flake"^^xsd:string,
        "Paul Ryan"^^xsd:string ;
    dct:description "An indication of 'necessity' within a context"@en ;
    rdfs:comment "Necessity can be used to express need, essentiality, requirement, or compulsion."@en ;
    rdfs:isDefinedBy dpvo: ;
    rdfs:subClassOf dpvo:Context ;
    sw:term_status "accepted"@en .

dpvo:ProcessingScale a owl:Class ;
    rdfs:label "Processing Scale"@en ;
    dct:created "2022-09-07"^^xsd:date ;
    dct:creator "Harshvardhan J. Pandit"^^xsd:string,
        "Piero Bonatti"^^xsd:string ;
    dct:description "Scale of Processing"@en ;
    rdfs:comment "The exact definition of what constitutes \"scale\" depends on use of jurisdictional, domain-specific, or other forms of externally defined criterias. Where possible, this should be reflected by extending the scales provided with the appropriate context."@en ;
    rdfs:isDefinedBy dpvo: ;
    rdfs:subClassOf dpvo:Scale ;
    sw:term_status "accepted"@en .

dpvo:Representative a owl:Class ;
    rdfs:label "Representative"@en ;
    dct:created "2020-11-04"^^xsd:date ;
    dct:creator "Beatriz Esteves"^^xsd:string,
        "Georg Krog"^^xsd:string,
        "Harshvardhan J. Pandit"^^xsd:string,
        "Paul Ryan"^^xsd:string ;
    dct:description "A representative of a legal entity"@en ;
    dct:source <https://eur-lex.europa.eu/eli/reg/2016/679/art_27/oj> ;
    rdfs:isDefinedBy dpvo: ;
    rdfs:subClassOf dpvo:LegalEntity ;
    sw:term_status "accepted"@en .

dpvo:ResearchAndDevelopment a owl:Class ;
    rdfs:label "Research and Development"@en ;
    dct:created "2019-04-05"^^xsd:date ;
    dct:creator "Axel Polleres"^^xsd:string,
        "Elmar Kiesling"^^xsd:string,
        "Fajar Ekaputra"^^xsd:string,
        "Harshvardhan J. Pandit"^^xsd:string,
        "Javier Fernandez"^^xsd:string,
        "Simon Steyskal"^^xsd:string ;
    dct:description "Purposes associated with conducting research and development for new methods, products, or services"@en ;
    rdfs:isDefinedBy dpvo: ;
    rdfs:subClassOf dpvo:Purpose ;
    sw:term_status "accepted"@en .

dpvo:SellProducts a owl:Class ;
    rdfs:label "Sell Products"@en ;
    dct:created "2021-09-08"^^xsd:date ;
    dct:creator "Beatriz Esteves"^^xsd:string,
        "Georg P Krog"^^xsd:string,
        "Harshvardhan J. Pandit"^^xsd:string ;
    dct:description "Purposes associated with selling products or services"@en ;
    rdfs:comment "Sell here means exchange, submit, or provide in return for direct or indirect compensation."@en ;
    rdfs:isDefinedBy dpvo: ;
    rdfs:subClassOf dpvo:ServiceProvision ;
    sw:term_status "accepted"@en .

dpvo:ServicePersonalisation a owl:Class ;
    rdfs:label "Service Personalisation"@en ;
    dct:created "2019-04-05"^^xsd:date ;
    dct:creator "Axel Polleres"^^xsd:string,
        "Elmar Kiesling"^^xsd:string,
        "Fajar Ekaputra"^^xsd:string,
        "Harshvardhan J. Pandit"^^xsd:string,
        "Javier Fernandez"^^xsd:string,
        "Simon Steyskal"^^xsd:string ;
    dct:description "Purposes associated with providing personalisation within services or product or activities"@en ;
    rdfs:isDefinedBy dpvo: ;
    rdfs:subClassOf dpvo:Personalisation,
        dpvo:ServiceProvision ;
    sw:term_status "accepted"@en .

dpvo:VendorManagement a owl:Class ;
    rdfs:label "Vendor Management"@en ;
    dct:created "2021-09-01"^^xsd:date ;
    dct:creator "David Hickey"^^xsd:string,
        "Georg P Krog"^^xsd:string,
        "Harshvardhan J. Pandit"^^xsd:string,
        "Paul Ryan"^^xsd:string ;
    dct:description "Purposes associated with manage orders, payment, evaluation, and prospecting related to vendors"@en ;
    dct:source <https://www.privacycommission.be/nl/model-voor-een-register-van-de-verwerkingsactiviteiten> ;
    rdfs:isDefinedBy dpvo: ;
    rdfs:subClassOf dpvo:Purpose ;
    sw:term_status "accepted"@en .

dpvo:VulnerableDataSubject a owl:Class ;
    rdfs:label "Vulnerable Data Subject"@en ;
    dct:created "2020-11-04"^^xsd:date ;
    dct:creator "Georg Krog"^^xsd:string,
        "Harshvardhan Pandit"^^xsd:string,
        "Paul Ryan"^^xsd:string ;
    dct:description "Data Subjects which should be considered 'vulnerable' and therefore would require additional measures and safeguards"@en ;
    rdfs:comment "This concept denotes a Data Subject or a group are vulnerable, but not what vulnerability they possess or its context. This information can be provided additionally as comments, or as separate concepts and relations. Proposals for this are welcome."@en ;
    rdfs:isDefinedBy dpvo: ;
    rdfs:subClassOf dpvo:DataSubject ;
    sw:term_status "accepted"@en .

dpvo:hasRule a rdf:Property,
        owl:ObjectProperty ;
    rdfs:label "has rule"@en ;
    dct:created "2022-10-19"^^xsd:date ;
    dct:creator "Beatriz Esteves"^^xsd:string,
        "Georg P Krog"^^xsd:string,
        "Harshvardhan J. Pandit"^^xsd:string,
        "Paul Ryan"^^xsd:string ;
    dct:description "Specifying applicability or inclusion of a rule within specified context"@en ;
    rdfs:domain dpvo:Context ;
    rdfs:isDefinedBy dpvo: ;
    rdfs:range dpvo:Rule ;
    sw:term_status "accepted"@en .

dpvo:hasScale a rdf:Property,
        owl:ObjectProperty ;
    rdfs:label "has scale"@en ;
    dct:created "2022-06-15"^^xsd:date ;
    dct:creator "Harshvardhan J. Pandit"^^xsd:string ;
    dct:description "Indicates the scale of specified concept"@en ;
    rdfs:domain owl:Thing ;
    rdfs:isDefinedBy dpvo: ;
    rdfs:range dpvo:Scale ;
    sw:term_status "accepted"@en .

dpvo:hasStatus a rdf:Property,
        owl:ObjectProperty ;
    rdfs:label "has status"@en ;
    dct:created "2022-05-18"^^xsd:date ;
    dct:creator "Harshvardhan J. Pandit"^^xsd:string ;
    dct:description "Indicates the status of specified concept"@en ;
    rdfs:domain owl:Thing ;
    rdfs:isDefinedBy dpvo: ;
    rdfs:range dpvo:Status ;
    sw:term_status "accepted"@en .

dpvo:CryptographicAuthentication a owl:Class ;
    rdfs:label "Cryptographic Authentication"@en ;
    dct:created "2022-08-17"^^xsd:date ;
    dct:creator "Harshvardhan J. Pandit"^^xsd:string ;
    dct:description "Use of cryptography for authentication"@en ;
    dct:source <https://www.enisa.europa.eu/publications/reference-incident-classification-taxonomy/> ;
    rdfs:isDefinedBy dpvo: ;
    rdfs:subClassOf dpvo:AuthenticationProtocols,
        dpvo:CryptographicMethods ;
    sw:term_status "accepted"@en .

dpvo:DataProcessingAgreement a owl:Class ;
    rdfs:label "Data Processing Agreement"@en ;
    dct:created "2022-01-26"^^xsd:date ;
    dct:creator "Beatriz Esteves"^^xsd:string,
        "Georg P Krog"^^xsd:string,
        "Harshvardhan J. Pandit"^^xsd:string,
        "Julian Flake"^^xsd:string,
        "Paul Ryan"^^xsd:string ;
    dct:description "An agreement outlining conditions, criteria, obligations, responsibilities, and specifics for carrying out processing of personal data"@en ;
    rdfs:comment "For specific role-based data processing agreements, see concepts for Processors and JointDataController agreements."@en ;
    rdfs:isDefinedBy dpvo: ;
    rdfs:subClassOf dpvo:LegalAgreement ;
    sw:term_status "accepted"@en .

dpvo:DataSource a owl:Class ;
    rdfs:label "Data Source"@en ;
    dct:created "2020-11-04"^^xsd:date ;
    dct:creator "Beatriz Esteves"^^xsd:string,
        "Georg P Krog"^^xsd:string,
        "Harshvardhan J. Pandit"^^xsd:string ;
    dct:description "The source or origin of data"@en ;
    rdfs:comment "Source' is the direct point of data collection; 'origin' would indicate the original/others points of where the data originates from."@en ;
    rdfs:isDefinedBy dpvo: ;
    rdfs:subClassOf dpvo:ProcessingContext ;
    sw:term_status "accepted"@en .

dpvo:EnforceSecurity a owl:Class ;
    rdfs:label "Enforce Security"@en ;
    dct:created "2019-04-05"^^xsd:date ;
    dct:creator "Axel Polleres"^^xsd:string,
        "Elmar Kiesling"^^xsd:string,
        "Fajar Ekaputra"^^xsd:string,
        "Harshvardhan J. Pandit"^^xsd:string,
        "Javier Fernandez"^^xsd:string,
        "Simon Steyskal"^^xsd:string ;
    dct:description "Purposes associated with ensuring and enforcing security for data, personnel, or other related matters"@en ;
    rdfs:comment "Was previous \"Security\". Prefixed to distinguish from TechOrg measures."@en ;
    rdfs:isDefinedBy dpvo: ;
    rdfs:subClassOf dpvo:Purpose ;
    sw:term_status "accepted"@en .

dpvo:HumanInvolvement a owl:Class ;
    rdfs:label "Human Involvement"@en ;
    dct:created "2022-01-26"^^xsd:date ;
    dct:creator "Harshvardhan J. Pandit"^^xsd:string ;
    dct:description "The involvement of humans in specified context"@en ;
    dct:modified "2022-06-15"^^xsd:date ;
    rdfs:comment "Human Involvement here broadly refers to any involvement by a human in the context of carrying out processing. This may include verification of outcomes, providing input data for making decisions, or overseeing activities."@en ;
    rdfs:isDefinedBy dpvo: ;
    rdfs:subClassOf dpvo:AutomationOfProcessing ;
    sw:term_status "accepted"@en .

dpvo:ImpactAssessment a owl:Class ;
    rdfs:label "Impact Assessment"@en ;
    dct:created "2020-11-04"^^xsd:date ;
    dct:creator "Georg P Krog"^^xsd:string,
        "Harshvardhan J. Pandit"^^xsd:string,
        "Paul Ryan"^^xsd:string ;
    dct:description "Calculating or determining the likelihood of impact of an existing or proposed process, which can involve risks or detriments."@en ;
    rdfs:isDefinedBy dpvo: ;
    rdfs:subClassOf dpvo:Assessment ;
    sw:term_status "accepted"@en .

dpvo:Lawfulness a owl:Class ;
    rdfs:label "Lawfulness"@en ;
    dct:created "2022-10-19"^^xsd:date ;
    dct:creator "Harshvardhan J. Pandit"^^xsd:string ;
    dct:description "Status associated with expressing lawfullness or legal compliance"@en ;
    rdfs:isDefinedBy dpvo: ;
    rdfs:subClassOf dpvo:ComplianceStatus ;
    sw:term_status "accepted"@en .

dpvo:LegalAgreement a owl:Class ;
    rdfs:label "Legal Agreement"@en ;
    dct:created "2019-04-05"^^xsd:date ;
    dct:creator "Axel Polleres"^^xsd:string,
        "Harshvardhan J. Pandit"^^xsd:string,
        "Mark Lizar"^^xsd:string,
        "Rob Brennan"^^xsd:string ;
    dct:description "A legally binding agreement"@en ;
    rdfs:isDefinedBy dpvo: ;
    rdfs:subClassOf dpvo:OrganisationalMeasure ;
    sw:term_status "accepted"@en .

dpvo:Marketing a owl:Class ;
    rdfs:label "Marketing"@en ;
    dct:created "2020-11-04"^^xsd:date ;
    dct:creator "Beatriz Esteves"^^xsd:string,
        "Georg P Krog"^^xsd:string,
        "Harshvardhan J. Pandit"^^xsd:string ;
    dct:description "Purposes associated with conducting marketing in relation to organisation or products or services e.g. promoting, selling, and distributing"@en ;
    rdfs:comment "Was commercial interest, changed to consider Marketing a separate Purpose category by itself"@en ;
    rdfs:isDefinedBy dpvo: ;
    rdfs:subClassOf dpvo:Purpose ;
    sw:term_status "accepted"@en .

dpvo:Notice a owl:Class ;
    rdfs:label "Notice"@en ;
    dct:created "2021-09-08"^^xsd:date ;
    dct:creator "David Hickey"^^xsd:string,
        "Georg P Krog"^^xsd:string,
        "Harshvardhan J. Pandit"^^xsd:string,
        "Paul Ryan"^^xsd:string ;
    dct:description "A notice is an artefact for providing information, choices, or controls"@en ;
    rdfs:isDefinedBy dpvo: ;
    rdfs:subClassOf dpvo:OrganisationalMeasure ;
    sw:term_status "accepted"@en .

dpvo:OptimisationForController a owl:Class ;
    rdfs:label "Optimisation for Controller"@en ;
    dct:created "2019-04-05"^^xsd:date ;
    dct:creator "Axel Polleres"^^xsd:string,
        "Elmar Kiesling"^^xsd:string,
        "Fajar Ekaputra"^^xsd:string,
        "Harshvardhan J. Pandit"^^xsd:string,
        "Javier Fernandez"^^xsd:string,
        "Simon Steyskal"^^xsd:string ;
    dct:description "Purposes associated with optimisation of activities and services for provider or controller"@en ;
    rdfs:isDefinedBy dpvo: ;
    rdfs:subClassOf dpvo:ServiceOptimisation ;
    sw:term_status "accepted"@en .

dpvo:OrganisationGovernance a owl:Class ;
    rdfs:label "Organisation Governance"@en ;
    dct:created "2021-09-01"^^xsd:date ;
    dct:creator "David Hickey"^^xsd:string,
        "Georg P Krog"^^xsd:string,
        "Harshvardhan J. Pandit"^^xsd:string,
        "Paul Ryan"^^xsd:string ;
    dct:description "Purposes associated with conducting activities and functions for governance of an organisation"@en ;
    dct:source <https://www.privacycommission.be/nl/model-voor-een-register-van-de-verwerkingsactiviteiten> ;
    rdfs:isDefinedBy dpvo: ;
    rdfs:subClassOf dpvo:Purpose ;
    sw:term_status "accepted"@en .

dpvo:Policy a owl:Class ;
    rdfs:label "Policy"@en ;
    dct:created "2021-09-08"^^xsd:date ;
    dct:creator "David Hickey"^^xsd:string,
        "Georg P Krog"^^xsd:string,
        "Harshvardhan J. Pandit"^^xsd:string,
        "Paul Ryan"^^xsd:string ;
    dct:description "A guidance document outlining any of: procedures, plans, principles, decisions, intent, or protocols."@en ;
    rdfs:isDefinedBy dpvo: ;
    rdfs:subClassOf dpvo:OrganisationalMeasure ;
    sw:term_status "accepted"@en .

dpvo:Recipient a owl:Class ;
    rdfs:label "Recipient"@en ;
    dct:created "2019-04-05"^^xsd:date ;
    dct:creator "Axel Polleres"^^xsd:string,
        "Javier Fernández"^^xsd:string ;
    dct:description "Entities that receive personal data"@en ;
    dct:modified "2020-11-04"^^xsd:date ;
    dct:source <https://eur-lex.europa.eu/eli/reg/2016/679/art_4/par_9/oj>,
        <https://specialprivacy.ercim.eu/> ;
    rdfs:comment "A recipient of personal data can be used to indicate any entity that receives personal data. This can be a Third Party, Processor (GDPR), or even a Controller."@en ;
    rdfs:isDefinedBy dpvo: ;
    rdfs:seeAlso spl:AnyRecipient ;
    rdfs:subClassOf dpvo:LegalEntity ;
    sw:term_status "accepted"@en .

dpvo:Right a owl:Class ;
    rdfs:label "Right"@en ;
    dct:created "2020-11-18"^^xsd:date ;
    dct:creator "Beatriz Esteves"^^xsd:string,
        "Georg P Krog"^^xsd:string,
        "Harshvardhan J Pandit"^^xsd:string ;
    dct:description "The right(s) applicable, provided, or expected"@en,
        "The right(s) applicable, provided, or expected."@en ;
    rdfs:comment "A 'right' is a legal, social, or ethical principle of freedom or entitlement which dictate the norms regarding what is allowed or owed.. Rights as a concept encompass a broad area of norms and entities, and are not specific to Individuals or Data Protection / Privacy. For individual specific rights, see dpv:DataSubjectRight"@en ;
    rdfs:isDefinedBy dpvo: ;
    sw:term_status "accepted"@en .

dpvo:Rule a owl:Class ;
    rdfs:label "Rule"@en ;
    dct:created "2022-10-19"^^xsd:date ;
    dct:creator "Beatriz Esteves"^^xsd:string,
        "Georg P Krog"^^xsd:string,
        "Harshvardhan J. Pandit"^^xsd:string,
        "Paul Ryan"^^xsd:string ;
    dct:description "A rule describing a process or control that directs or determines if and how an activity should be conducted"@en ;
    rdfs:isDefinedBy dpvo: ;
    sw:term_status "accepted"@en .

dpvo:TechnicalOrganisationalMeasure a owl:Class ;
    rdfs:label "Technical and Organisational Measure"@en ;
    dct:created "2019-04-05"^^xsd:date ;
    dct:creator "Bud Bruegger"^^xsd:string ;
    dct:description "The Technical and Organisational measures used."@en ;
    dct:modified "2020-11-04"^^xsd:date ;
    rdfs:isDefinedBy dpvo: ;
    sw:term_status "accepted"@en .

dpvo:hasRecipient a rdf:Property,
        owl:ObjectProperty ;
    rdfs:label "has recipient"@en ;
    dct:created "2019-04-04"^^xsd:date ;
    dct:creator "Axel Polleres"^^xsd:string,
        "Bud Bruegger"^^xsd:string,
        "Harshvardhan J. Pandit"^^xsd:string,
        "Javier Fernández"^^xsd:string,
        "Mark Lizar"^^xsd:string ;
    dct:description "Indicates Recipient of Personal Data"@en ;
    dct:modified "2020-11-04"^^xsd:date ;
    dct:source <https://specialprivacy.ercim.eu/> ;
    rdfs:domain owl:Thing ;
    rdfs:isDefinedBy dpvo: ;
    rdfs:range dpvo:Recipient ;
    rdfs:subPropertyOf dpvo:hasEntity ;
    sw:term_status "accepted"@en .

dpvo:hasTechnicalOrganisationalMeasure a rdf:Property,
        owl:ObjectProperty ;
    rdfs:label "has technical and organisational measure"@en ;
    dct:created "2019-04-04"^^xsd:date ;
    dct:creator "Axel Polleres"^^xsd:string,
        "Bud Bruegger"^^xsd:string,
        "Harshvardhan J. Pandit"^^xsd:string,
        "Javier Fernández"^^xsd:string,
        "Mark Lizar"^^xsd:string ;
    dct:description "Indicates use or applicability of Technical or Organisational measure"@en ;
    dct:modified "2020-11-04"^^xsd:date ;
    rdfs:domain owl:Thing ;
    rdfs:isDefinedBy dpvo: ;
    rdfs:range dpvo:TechnicalOrganisationalMeasure ;
    sw:term_status "accepted"@en .

dpvo:Assessment a owl:Class ;
    rdfs:label "Assessment"@en ;
    dct:created "2021-09-08"^^xsd:date ;
    dct:creator "Harshvardhan J. Pandit"^^xsd:string ;
    dct:description "The document, plan, or process for assessment or determination towards a purpose e.g. assessment of legality or impact assessments"@en ;
    rdfs:isDefinedBy dpvo: ;
    rdfs:subClassOf dpvo:OrganisationalMeasure ;
    sw:term_status "accepted"@en .

dpvo:CustomerManagement a owl:Class ;
    rdfs:label "Customer Management"@en ;
    dct:created "2021-09-08"^^xsd:date ;
    dct:creator "Beatriz"^^xsd:string,
        "Georg P Krog"^^xsd:string,
        "Harshvardhan J. Pandit"^^xsd:string ;
    dct:description "Customer Management refers to purposes associated with managing activities related with past, current, and future customers"@en ;
    rdfs:isDefinedBy dpvo: ;
    rdfs:subClassOf dpvo:Purpose ;
    sw:term_status "accepted"@en .

dpvo:Disclose a owl:Class ;
    rdfs:label "Disclose"@en ;
    dct:created "2019-05-07"^^xsd:date ;
    dct:description "to make data known"@en ;
    dct:source <https://eur-lex.europa.eu/eli/reg/2016/679/art_4/par_2/oj> ;
    rdfs:isDefinedBy dpvo: ;
    rdfs:subClassOf dpvo:Processing ;
    sw:term_status "accepted"@en .

dpvo:Frequency a owl:Class ;
    rdfs:label "Frequency"@en ;
    dct:created "2022-02-16"^^xsd:date ;
    dct:creator "Harshvardhan J. Pandit"^^xsd:string ;
    dct:description "The frequency or information about periods and repetitions in terms of recurrence."@en ;
    rdfs:isDefinedBy dpvo: ;
    rdfs:subClassOf dpvo:Context ;
    sw:term_status "accepted"@en .

dpvo:Impact a owl:Class ;
    rdfs:label "Impact"@en ;
    dct:created "2022-03-23"^^xsd:date ;
    dct:creator "Beatriz Esteves"^^xsd:string,
        "Fajar Ekaputra"^^xsd:string,
        "Georg P Krog"^^xsd:string,
        "Harshvardhan J. Pandit"^^xsd:string,
        "Julian Flake"^^xsd:string ;
    dct:description "The impact(s) possible or arising as a consequence from specified context"@en ;
    rdfs:comment "Impact is a stronger notion of consequence in terms of influence, change, or effect on something e.g. for impact assessments"@en ;
    rdfs:isDefinedBy dpvo: ;
    rdfs:subClassOf dpvo:Consequence ;
    sw:term_status "accepted"@en .

dpvo:LocalLocation a owl:Class ;
    rdfs:label "Local Location"@en ;
    dct:created "2022-06-15"^^xsd:date ;
    dct:creator "Harshvardhan J. Pandit"^^xsd:string ;
    dct:description "Location is local"@en ;
    dct:modified "2020-10-05"^^xsd:date ;
    rdfs:isDefinedBy dpvo: ;
    rdfs:subClassOf dpvo:LocationLocality ;
    sw:term_status "modified"@en .

dpvo:LocationFixture a owl:Class ;
    rdfs:label "Location Fixture"@en ;
    dct:created "2022-06-15"^^xsd:date ;
    dct:creator "Harshvardhan J. Pandit"^^xsd:string ;
    dct:description "The fixture of location refers to whether the location is fixed"@en ;
    rdfs:isDefinedBy dpvo: ;
    sw:term_status "accepted"@en .

dpvo:Pseudonymisation a owl:Class ;
    rdfs:label "Pseudonymisation"@en ;
    dct:created "2019-04-05"^^xsd:date ;
    dct:creator "Axel Polleres"^^xsd:string,
        "Harshvardhan J. Pandit"^^xsd:string,
        "Mark Lizar"^^xsd:string,
        "Rob Brennan"^^xsd:string ;
    dct:description "Pseudonymisation means the processing of personal data in such a manner that the personal data can no longer be attributed to a specific data subject without the use of additional information, provided that such additional information is kept separately and is subject to technical and organisational measures to ensure that the personal data are not attributed to an identified or identifiable natural person;"@en ;
    dct:modified "2022-11-24"^^xsd:date ;
    dct:source <https://eur-lex.europa.eu/eli/reg/2016/679/art_4/par_5/oj> ;
    rdfs:isDefinedBy dpvo: ;
    rdfs:subClassOf dpvo:Deidentification ;
    sw:term_status "modified"@en .

dpvo:Scale a owl:Class ;
    rdfs:label "Scale"@en ;
    dct:created "2022-06-15"^^xsd:date ;
    dct:creator "Georg P Krog"^^xsd:string,
        "Harshvardhan J. Pandit"^^xsd:string,
        "Rana Saniei"^^xsd:string ;
    dct:description "A measurement along some dimension"@en ;
    rdfs:comment "Scales are subjective concepts that need to be defined and interpreted within the context of their application. For example, what would be small within one context could be large within another."@en ;
    rdfs:isDefinedBy dpvo: ;
    rdfs:subClassOf dpvo:ProcessingContext ;
    sw:term_status "accepted"@en .

dpvo:StaffTraining a owl:Class ;
    rdfs:label "Staff Training"@en ;
    dct:created "2019-04-05"^^xsd:date ;
    dct:creator "Axel Polleres"^^xsd:string,
        "Harshvardhan J. Pandit"^^xsd:string,
        "Mark Lizar"^^xsd:string,
        "Rob Brennan"^^xsd:string ;
    dct:description "Practices and policies regarding training of staff members"@en ;
    rdfs:isDefinedBy dpvo: ;
    rdfs:subClassOf dpvo:OrganisationalMeasure ;
    sw:term_status "accepted"@en .

dpvo:StorageCondition a owl:Class ;
    rdfs:label "Storage Condition"@en ;
    dct:created "2019-04-05"^^xsd:date ;
    dct:creator "Axel Polleres"^^xsd:string,
        "Harshvardhan J. Pandit"^^xsd:string,
        "Mark Lizar"^^xsd:string,
        "Rob Brennan"^^xsd:string ;
    dct:description "Conditions required or followed regarding storage of data"@en ;
    rdfs:isDefinedBy dpvo: ;
    rdfs:subClassOf dpvo:ProcessingContext ;
    sw:term_status "accepted"@en .

dpvo:ActivityStatus a owl:Class ;
    rdfs:label "Activity Status"@en ;
    dct:created "2022-05-18"^^xsd:date ;
    dct:creator "Harshvardhan J. Pandit"^^xsd:string ;
    dct:description "Status associated with activity operations and lifecycles"@en ;
    rdfs:isDefinedBy dpvo: ;
    rdfs:subClassOf dpvo:Status ;
    sw:term_status "accepted"@en .

dpvo:AuthenticationProtocols a owl:Class ;
    rdfs:label "Authentication Protocols"@en ;
    dct:created "2019-04-05"^^xsd:date ;
    dct:creator "Axel Polleres"^^xsd:string,
        "Harshvardhan J. Pandit"^^xsd:string,
        "Mark Lizar"^^xsd:string,
        "Rob Brennan"^^xsd:string ;
    dct:description "Protocols involving validation of identity i.e. authentication of a person or information"@en ;
    rdfs:isDefinedBy dpvo: ;
    rdfs:subClassOf dpvo:TechnicalMeasure ;
    sw:term_status "accepted"@en .

dpvo:Authority a owl:Class ;
    rdfs:label "Authority"@en ;
    dct:created "2020-11-04"^^xsd:date ;
    dct:creator "Georg Krog"^^xsd:string,
        "Harshvardhan Pandit"^^xsd:string,
        "Paul Ryan"^^xsd:string ;
    dct:description "An authority with the power to create or enforce laws, or determine their compliance."@en ;
    rdfs:isDefinedBy dpvo: ;
    rdfs:subClassOf dpvo:GovernmentalOrganisation,
        dpvo:LegalEntity ;
    sw:term_status "accepted"@en .

dpvo:Consequence a owl:Class ;
    rdfs:label "Consequence"@en ;
    dct:created "2022-01-26"^^xsd:date ;
    dct:creator "Harshvardhan J. Pandit"^^xsd:string ;
    dct:description "The consequence(s) possible or arising from specified context"@en ;
    rdfs:isDefinedBy dpvo: ;
    sw:term_status "accepted"@en .

dpvo:Encryption a owl:Class ;
    rdfs:label "Encryption"@en ;
    dct:created "2019-04-05"^^xsd:date ;
    dct:creator "Axel Polleres"^^xsd:string,
        "Harshvardhan J. Pandit"^^xsd:string,
        "Mark Lizar"^^xsd:string,
        "Rob Brennan"^^xsd:string ;
    dct:description "Technical measures consisting of encryption"@en ;
    rdfs:isDefinedBy dpvo: ;
    rdfs:subClassOf dpvo:TechnicalMeasure ;
    sw:term_status "accepted"@en .

dpvo:Obtain a owl:Class ;
    rdfs:label "Obtain"@en ;
    dct:created "2019-05-07"^^xsd:date ;
    dct:description "to solicit or gather data from someone"@en ;
    dct:source <https://eur-lex.europa.eu/eli/reg/2016/679/art_4/par_2/oj> ;
    rdfs:isDefinedBy dpvo: ;
    rdfs:subClassOf dpvo:Processing ;
    sw:term_status "accepted"@en .

dpvo:PersonalData a owl:Class ;
    rdfs:label "Personal Data"@en ;
    dct:created "2019-04-05"^^xsd:date ;
    dct:creator "Harshvardhan Pandit"^^xsd:string ;
    dct:description "Data directly or indirectly associated or related to an individual."@en ;
    dct:modified "2022-01-19"^^xsd:date ;
    dct:source <https://eur-lex.europa.eu/eli/reg/2016/679/art_4/par_1/oj> ;
    rdfs:comment "This definition of personal data encompasses the concepts used in GDPR Art.4-1 for 'personal data' and ISO/IEC 2700 for 'personally identifiable information (PII)'."@en ;
    rdfs:isDefinedBy dpvo: ;
    rdfs:seeAlso spl:AnyData ;
    rdfs:subClassOf dpvo:Data ;
    sw:term_status "accepted"@en .

dpvo:AuditStatus a owl:Class ;
    rdfs:label "Audit Status"@en ;
    dct:created "2022-05-18"^^xsd:date ;
    dct:creator "Harshvardhan J. Pandit"^^xsd:string ;
    dct:description "Status associated with Auditing or Investigation"@en ;
    rdfs:isDefinedBy dpvo: ;
    rdfs:subClassOf dpvo:Status ;
    sw:term_status "accepted"@en .

dpvo:Data a owl:Class ;
    rdfs:label "Data"@en ;
    dct:created "2022-01-19"^^xsd:date ;
    dct:creator "Harshvardhan J. Pandit"^^xsd:string ;
    dct:description "A broad concept representing  'data' or 'information'"@en ;
    rdfs:isDefinedBy dpvo: ;
    sw:term_status "accepted"@en .

dpvo:DataSubjectScale a owl:Class ;
    rdfs:label "Data Subject Scale"@en ;
    dct:created "2022-06-15"^^xsd:date ;
    dct:creator "Georg P Krog"^^xsd:string,
        "Harshvardhan J. Pandit"^^xsd:string,
        "Rana Saniei"^^xsd:string ;
    dct:description "Scale of Data Subject(s)"@en ;
    rdfs:isDefinedBy dpvo: ;
    rdfs:subClassOf dpvo:Scale ;
    sw:term_status "accepted"@en .

dpvo:DataVolume a owl:Class ;
    rdfs:label "Data Volume"@en ;
    dct:created "2022-06-15"^^xsd:date ;
    dct:creator "Georg P Krog"^^xsd:string,
        "Harshvardhan J. Pandit"^^xsd:string,
        "Rana Saniei"^^xsd:string ;
    dct:description "Volume or Scale of Data"@en ;
    rdfs:isDefinedBy dpvo: ;
    rdfs:subClassOf dpvo:Scale ;
    sw:term_status "accepted"@en .

dpvo:GovernanceProcedures a owl:Class ;
    rdfs:label "Governance Procedures"@en ;
    dct:created "2022-08-17"^^xsd:date ;
    dct:creator "Harshvardhan J. Pandit"^^xsd:string ;
    dct:description "Procedures related to governance (e.g. organisation, unit, team, process, system)"@en ;
    dct:source <https://www.enisa.europa.eu/publications/5g-cybersecurity-standards> ;
    rdfs:isDefinedBy dpvo: ;
    rdfs:subClassOf dpvo:OrganisationalMeasure ;
    sw:term_status "accepted"@en .

dpvo:Organisation a owl:Class ;
    rdfs:label "Organisation"@en ;
    dct:created "2022-02-02"^^xsd:date ;
    dct:creator "Harshvardhan J. Pandit"^^xsd:string ;
    dct:description "A general term reflecting a company or a business or a group acting as a unit"@en ;
    rdfs:isDefinedBy dpvo: ;
    rdfs:subClassOf dpvo:LegalEntity ;
    sw:term_status "accepted"@en .

dpvo:Status a owl:Class ;
    rdfs:label "Status"@en ;
    dct:created "2022-05-18"^^xsd:date ;
    dct:creator "Harshvardhan J. Pandit"^^xsd:string ;
    dct:description "The status or state of something"@en ;
    rdfs:isDefinedBy dpvo: ;
    rdfs:subClassOf dpvo:Context ;
    sw:term_status "accepted"@en .

dpvo:Use a owl:Class ;
    rdfs:label "Use"@en ;
    dct:created "2019-05-07"^^xsd:date ;
    dct:description "to use data"@en ;
    dct:source <https://eur-lex.europa.eu/eli/reg/2016/679/art_4/par_2/oj> ;
    rdfs:isDefinedBy dpvo: ;
    rdfs:subClassOf dpvo:Processing ;
    sw:term_status "accepted"@en .

dpvo:ComplianceStatus a owl:Class ;
    rdfs:label "Compliance Status"@en ;
    dct:created "2022-05-18"^^xsd:date ;
    dct:creator "Harshvardhan J. Pandit"^^xsd:string ;
    dct:description "Status associated with Compliance with some norms, objectives, or requirements"@en ;
    rdfs:isDefinedBy dpvo: ;
    rdfs:subClassOf dpvo:Status ;
    sw:term_status "accepted"@en .

dpvo:ConsentStatusInvalidForProcessing a owl:Class ;
    rdfs:label "Consent Status Invalid for Processing"@en ;
    dct:created "2022-06-22"^^xsd:date ;
    dct:creator "Georg P Krog"^^xsd:string,
        "Harshvardhan J. Pandit"^^xsd:string,
        "Julian Flake"^^xsd:string,
        "Paul Ryan"^^xsd:string ;
    dct:description "States of consent that cannot be used as valid justifications for processing data"@en ;
    dct:source <https://w3id.org/GConsent> ;
    rdfs:comment "This identifies the stages associated with consent that should not be used to process data"@en ;
    rdfs:isDefinedBy dpvo: ;
    rdfs:subClassOf dpvo:ConsentStatus ;
    sw:term_status "accepted"@en .

dpvo:Duration a owl:Class ;
    rdfs:label "Duration"@en ;
    dct:created "2022-02-09"^^xsd:date ;
    dct:creator "Harshvardhan J. Pandit"^^xsd:string ;
    dct:description "The duration or temporal limitation"@en ;
    rdfs:isDefinedBy dpvo: ;
    rdfs:subClassOf dpvo:Context ;
    sw:term_status "accepted"@en .

dpvo:GeographicCoverage a owl:Class ;
    rdfs:label "Geographic Coverage"@en ;
    dct:created "2022-06-15"^^xsd:date ;
    dct:creator "Georg P Krog"^^xsd:string,
        "Harshvardhan J. Pandit"^^xsd:string,
        "Paul Ryan"^^xsd:string ;
    dct:description "Indicate of scale in terms of geographic coverage"@en ;
    rdfs:isDefinedBy dpvo: ;
    rdfs:subClassOf dpvo:Scale ;
    sw:term_status "accepted"@en .

dpvo:LegalEntity a owl:Class ;
    rdfs:label "Legal Entity"@en ;
    dct:created "2019-04-05"^^xsd:date ;
    dct:creator "Harshvardhan J. Pandit"^^xsd:string ;
    dct:description "A human or non-human 'thing' that constitutes as an entity and which is recognised and defined in law"@en ;
    rdfs:isDefinedBy dpvo: ;
    rdfs:subClassOf dpvo:Entity ;
    sw:term_status "accepted"@en .

dpvo:ProcessingContext a owl:Class ;
    rdfs:label "Processing Context"@en ;
    dct:created "2022-02-09"^^xsd:date ;
    dct:creator "Harshvardhan J. Pandit"^^xsd:string ;
    dct:description "Context or conditions within which processing takes place"@en ;
    rdfs:isDefinedBy dpvo: ;
    rdfs:subClassOf dpvo:Context ;
    sw:term_status "accepted"@en .

dpvo:Risk a owl:Class ;
    rdfs:label "Risk"@en ;
    dct:created "2020-11-18"^^xsd:date ;
    dct:creator "Harshvardhan J. Pandit"^^xsd:string ;
    dct:description "A risk or possibility or uncertainty of negative effects, impacts, or consequences."@en ;
    rdfs:comment "Risks can be associated with one or more different concepts such as purpose, processing, personal data, technical or organisational measure."@en ;
    rdfs:isDefinedBy dpvo: ;
    sw:term_status "accepted"@en .

dpvo:SecurityProcedure a owl:Class ;
    rdfs:label "Security Procedure"@en ;
    dct:created "2022-08-24"^^xsd:date ;
    dct:creator "Harshvardhan J. Pandit"^^xsd:string ;
    dct:description "Procedures associated with assessing, implementing, and evaluating security"@en ;
    rdfs:isDefinedBy dpvo: ;
    rdfs:subClassOf dpvo:OrganisationalMeasure ;
    sw:term_status "accepted"@en .

dpvo:hasEntity a rdf:Property,
        owl:ObjectProperty ;
    rdfs:label "has entity"@en ;
    dct:created "2022-02-09"^^xsd:date ;
    dct:creator "Harshvardhan J. Pandit"^^xsd:string ;
    dct:description "Indicates inclusion or applicability of an entity to some concept"@en ;
    rdfs:comment "parent property for controller, processor, data subject, authority, etc.?"@en ;
    rdfs:domain owl:Thing ;
    rdfs:isDefinedBy dpvo: ;
    rdfs:range dpvo:Entity ;
    sw:term_status "accepted"@en .

dpvo:LegalBasis a owl:Class ;
    rdfs:label "Legal Basis"@en ;
    dct:created "2019-04-05"^^xsd:date ;
    dct:creator "Axel Polleres"^^xsd:string,
        "Javier Fernández"^^xsd:string ;
    dct:description "The Legal basis used to justify processing of personal data"@en ;
    dct:modified "2020-11-04"^^xsd:date ;
    rdfs:comment "Legal basis (plural: legal bases) are defined by legislations and regulations, whose applicability is usually restricted to specific jurisdictions."@en ;
    rdfs:isDefinedBy dpvo: ;
    sw:term_status "accepted"@en .

dpvo:Location a owl:Class ;
    rdfs:label "Location"@en ;
    dct:created "2022-01-19"^^xsd:date ;
    dct:creator "Georg P Krog"^^xsd:string,
        "Harshvardhan J. Pandit"^^xsd:string ;
    dct:description "A location is a position, site, or area where something is located"@en ;
    rdfs:comment "Location may be geographic, physical, or virtual."@en ;
    rdfs:isDefinedBy dpvo: ;
    sw:term_status "accepted"@en .

dpvo:Transform a owl:Class ;
    rdfs:label "Transform"@en ;
    dct:created "2019-05-07"^^xsd:date ;
    dct:description "to change the form or nature of data"@en ;
    dct:source <https://eur-lex.europa.eu/eli/reg/2016/679/art_4/par_2/oj> ;
    rdfs:isDefinedBy dpvo: ;
    rdfs:subClassOf dpvo:Processing ;
    sw:term_status "accepted"@en .

dpvo:AutomationOfProcessing a owl:Class ;
    rdfs:label "Automation of Processing"@en ;
    dct:created "2022-06-15"^^xsd:date ;
    dct:creator "Harshvardhan J. Pandit"^^xsd:string ;
    dct:description "Contextual information about the degree of automation and human involvement associated with Processing"@en ;
    rdfs:comment "It is difficult to provide a formal definition of automation since any and all processing may be considered automation. This concept instead is intended to explicitly signal the utilisation of automation and its extent towards some context - such as decision making, and to indicate the involvement of humans."@en ;
    rdfs:isDefinedBy dpvo: ;
    rdfs:subClassOf dpvo:ProcessingContext ;
    sw:term_status "accepted"@en .

dpvo:Processing a owl:Class ;
    rdfs:label "Processing"@en ;
    dct:created "2019-04-05"^^xsd:date ;
    dct:creator "Axel Polleres"^^xsd:string,
        "Javier Fernández"^^xsd:string ;
    dct:description "The processing performed on personal data"@en ;
    dct:modified "2020-11-04"^^xsd:date ;
    dct:source <https://specialprivacy.ercim.eu/> ;
    rdfs:isDefinedBy dpvo: ;
    rdfs:seeAlso spl:AnyProcessing ;
    sw:term_status "accepted"@en .

dpvo:RequestStatus a owl:Class ;
    rdfs:label "Request Status"@en ;
    dct:created "2022-11-30"^^xsd:date ;
    dct:creator "Harshvardhan J. Pandit"^^xsd:string ;
    dct:description "Status associated with requests"@en ;
    rdfs:isDefinedBy dpvo: ;
    rdfs:subClassOf dpvo:Status ;
    sw:term_status "accepted"@en .

dpvo:ServiceProvision a owl:Class ;
    rdfs:label "Service Provision"@en ;
    dct:created "2019-04-05"^^xsd:date ;
    dct:creator "Axel Polleres"^^xsd:string,
        "Elmar Kiesling"^^xsd:string,
        "Fajar Ekaputra"^^xsd:string,
        "Harshvardhan J. Pandit"^^xsd:string,
        "Javier Fernandez"^^xsd:string,
        "Simon Steyskal"^^xsd:string ;
    dct:description "Purposes associated with providing service or product or activities"@en ;
    rdfs:isDefinedBy dpvo: ;
    rdfs:subClassOf dpvo:Purpose ;
    sw:term_status "accepted"@en .

dpvo:TechnicalMeasure a owl:Class ;
    rdfs:label "Technical Measure"@en ;
    dct:created "2019-04-05"^^xsd:date ;
    dct:creator "Axel Polleres"^^xsd:string,
        "Harshvardhan J. Pandit"^^xsd:string,
        "Mark Lizar"^^xsd:string,
        "Rob Brennan"^^xsd:string ;
    dct:description "Technical measures required/followed when processing data of the declared category"@en ;
    rdfs:isDefinedBy dpvo: ;
    rdfs:subClassOf dpvo:TechnicalOrganisationalMeasure ;
    sw:term_status "accepted"@en .

dpvo:Context a owl:Class ;
    rdfs:label "Context"@en ;
    dct:created "2019-04-05"^^xsd:date ;
    dct:creator "Axel Polleres"^^xsd:string,
        "Elmar Kiesling"^^xsd:string,
        "Fajar Ekaputra"^^xsd:string,
        "Harshvardhan J. Pandit"^^xsd:string,
        "Javier Fernandez"^^xsd:string,
        "Simon Steyskal"^^xsd:string ;
    dct:description "Contextually relevant information not possible to represent through other core concepts"@en ;
    dct:modified "2022-06-15"^^xsd:date ;
    rdfs:isDefinedBy dpvo: ;
    sw:term_status "modified"@en .

dpvo:Entity a owl:Class ;
    rdfs:label "Entity"@en ;
    dct:created "2022-02-02"^^xsd:date ;
    dct:creator "Harshvardhan J. Pandit"^^xsd:string ;
    dct:description "A human or non-human 'thing' that constitutes as an entity"@en ;
    rdfs:isDefinedBy dpvo: ;
    sw:term_status "accepted"@en .

dpvo:Purpose a owl:Class ;
    rdfs:label "Purpose"@en ;
    dct:created "2019-04-05"^^xsd:date ;
    dct:creator "Axel Polleres"^^xsd:string,
        "Javier Fernández"^^xsd:string ;
    dct:description "The purpose of processing personal data"@en ;
    dct:modified "2020-11-04"^^xsd:date ;
    dct:source <https://specialprivacy.ercim.eu/> ;
    vann:example dex:E0004 ;
    rdfs:isDefinedBy dpvo: ;
    rdfs:seeAlso spl:AnyPurpose ;
    sw:term_status "accepted"@en .

dpvo:SecurityMethod a owl:Class ;
    rdfs:label "Security Method"@en ;
    dct:created "2022-08-24"^^xsd:date ;
    dct:creator "Harshvardhan J. Pandit"^^xsd:string ;
    dct:description "Methods that relate to creating and providing security"@en ;
    rdfs:isDefinedBy dpvo: ;
    rdfs:subClassOf dpvo:TechnicalMeasure ;
    sw:term_status "accepted"@en .

dpvo:CryptographicMethods a owl:Class ;
    rdfs:label "Cryptographic Methods"@en ;
    dct:created "2022-08-17"^^xsd:date ;
    dct:creator "Harshvardhan J. Pandit"^^xsd:string ;
    dct:description "Use of cryptographic methods to perform tasks"@en ;
    dct:source <https://www.enisa.europa.eu/publications/reference-incident-classification-taxonomy/> ;
    rdfs:isDefinedBy dpvo: ;
    rdfs:subClassOf dpvo:TechnicalMeasure ;
    sw:term_status "accepted"@en .

dpvo:OrganisationalMeasure a owl:Class ;
    rdfs:label "Organisational Measure"@en ;
    dct:created "2019-04-05"^^xsd:date ;
    dct:creator "Axel Polleres"^^xsd:string,
        "Harshvardhan J. Pandit"^^xsd:string,
        "Mark Lizar"^^xsd:string,
        "Rob Brennan"^^xsd:string ;
    dct:description "Organisational measures required/followed when processing data of the declared category"@en ;
    rdfs:isDefinedBy dpvo: ;
    rdfs:subClassOf dpvo:TechnicalOrganisationalMeasure ;
    sw:term_status "accepted"@en .

dpvo:DataSubject a owl:Class ;
    rdfs:label "Data Subject"@en ;
    dct:created "2019-04-05"^^xsd:date ;
    dct:creator "Axel Polleres"^^xsd:string,
        "Javier Fernández"^^xsd:string ;
    dct:description "The individual (or category of individuals) whose personal data is being processed"@en ;
    dct:modified "2020-11-04"^^xsd:date ;
    dct:source <https://eur-lex.europa.eu/eli/reg/2016/679/art_4/par_1/oj> ;
    rdfs:comment "The term 'data subject' is specific to the GDPR, but is functionally equivalent to the term 'individual' and the ISO/IEC term 'PII Principle'."@en ;
    rdfs:isDefinedBy dpvo: ;
    rdfs:subClassOf dpvo:LegalEntity,
        dpvo:NaturalPerson ;
    sw:term_status "accepted"@en .

