@prefix ai: <https://w3id.org/dpv/ai#> .
@prefix bibo: <http://purl.org/ontology/bibo/> .
@prefix dct: <http://purl.org/dc/terms/> .
@prefix foaf: <http://xmlns.com/foaf/0.1/> .
@prefix org: <http://www.w3.org/ns/org#> .
@prefix owl: <http://www.w3.org/2002/07/owl#> .
@prefix profile: <http://www.w3.org/ns/dx/prof/> .
@prefix rdfs: <http://www.w3.org/2000/01/rdf-schema#> .
@prefix role: <http://www.w3.org/ns/dx/prof/role/> .
@prefix schema: <https://schema.org/> .
@prefix scoro: <http://purl.org/spar/scoro/> .
@prefix skos: <http://www.w3.org/2004/02/skos/core#> .
@prefix sw: <http://www.w3.org/2003/06/sw-vocab-status/ns#> .
@prefix tech: <https://w3id.org/dpv/tech#> .
@prefix vann: <http://purl.org/vocab/vann/> .
@prefix xsd: <http://www.w3.org/2001/XMLSchema#> .

ai:ContinuousValidationStage a rdfs:Class,
        skos:Concept,
        ai:LifecycleStage ;
    dct:contributor _:person-delaram-golpayegani ;
    dct:created "2024-12-01"^^xsd:date ;
    dct:source "ISO/IEC 22989:2022"@en ;
    rdfs:isDefinedBy ai: ;
    sw:term_status "accepted"@en ;
    skos:broader ai:LifecycleStage ;
    skos:definition "The stage in the lifecycle where there is continuous learning within the AI system by incremental training on an ongoing basis while the system is running in production"@en ;
    skos:inScheme ai:lifecycle-classes ;
    skos:prefLabel "Continuous Validation Stage"@en .

ai:DecommissionStage a rdfs:Class,
        skos:Concept,
        ai:LifecycleStage ;
    dct:contributor _:person-arthit-suriyawongkul,
        _:person-harshvardhan-j-pandit ;
    dct:created "2024-12-01"^^xsd:date ;
    dct:modified "2025-08-06"^^xsd:date ;
    dct:source "ISO/IEC 22989:2022"@en ;
    rdfs:isDefinedBy ai: ;
    sw:term_status "modified"@en ;
    skos:broader ai:RetirementStage ;
    skos:definition "The stage in the lifecycle where the AI system is being decommissioned as part of retirement"@en ;
    skos:inScheme ai:lifecycle-classes ;
    skos:prefLabel "Decommission Stage"@en .

ai:DeploymentStage a rdfs:Class,
        skos:Concept,
        ai:LifecycleStage ;
    dct:contributor _:person-delaram-golpayegani ;
    dct:created "2024-12-01"^^xsd:date ;
    dct:source "ISO/IEC 22989:2022"@en ;
    rdfs:isDefinedBy ai: ;
    sw:term_status "accepted"@en ;
    skos:broader ai:LifecycleStage ;
    skos:definition "The stage in the lifecycle where the AI system is installed, released or configured for deployment and operation in a target environment"@en ;
    skos:inScheme ai:lifecycle-classes ;
    skos:prefLabel "Deployment Stage"@en .

ai:DesignStage a rdfs:Class,
        skos:Concept,
        ai:LifecycleStage ;
    dct:contributor _:person-delaram-golpayegani ;
    dct:created "2024-12-01"^^xsd:date ;
    dct:source "ISO/IEC 22989:2022"@en ;
    rdfs:isDefinedBy ai: ;
    sw:term_status "accepted"@en ;
    skos:broader ai:LifecycleStage ;
    skos:definition "The stage in the lifecycle where designs are created for the AI system"@en ;
    skos:inScheme ai:lifecycle-classes ;
    skos:prefLabel "Design Stage"@en .

ai:DevelopmentStage a rdfs:Class,
        skos:Concept,
        ai:LifecycleStage ;
    dct:contributor _:person-delaram-golpayegani ;
    dct:created "2024-12-01"^^xsd:date ;
    dct:source "ISO/IEC 22989:2022"@en ;
    rdfs:isDefinedBy ai: ;
    sw:term_status "accepted"@en ;
    skos:broader ai:LifecycleStage ;
    skos:definition "The stage in the lifecycle where the development and creation of the system occurs, signalling upon completion that it is ready for verification and validation"@en ;
    skos:inScheme ai:lifecycle-classes ;
    skos:prefLabel "Development Stage"@en .

ai:DiscardStage a rdfs:Class,
        skos:Concept,
        ai:LifecycleStage ;
    dct:contributor _:person-harshvardhan-j-pandit ;
    dct:created "2024-12-01"^^xsd:date ;
    dct:source "ISO/IEC 22989:2022"@en ;
    rdfs:isDefinedBy ai: ;
    sw:term_status "accepted"@en ;
    skos:broader ai:RetirementStage ;
    skos:definition "The stage in the lifecycle where the AI system is being discarded as part of retirement"@en ;
    skos:inScheme ai:lifecycle-classes ;
    skos:prefLabel "Discard Stage"@en .

ai:InceptionStage a rdfs:Class,
        skos:Concept,
        ai:LifecycleStage ;
    dct:contributor _:person-delaram-golpayegani ;
    dct:created "2024-12-01"^^xsd:date ;
    dct:source "ISO/IEC 22989:2022"@en ;
    rdfs:isDefinedBy ai: ;
    sw:term_status "accepted"@en ;
    skos:broader ai:LifecycleStage ;
    skos:definition "The stage in the lifecycle where inception regarding AI occurs and one or more stakeholders decide to turn an idea into a tangible system"@en ;
    skos:inScheme ai:lifecycle-classes ;
    skos:prefLabel "Inception Stage"@en .

ai:IncidentMonitoringStage a rdfs:Class,
        skos:Concept,
        ai:LifecycleStage ;
    dct:contributor _:person-harshvardhan-j-pandit ;
    dct:created "2024-12-01"^^xsd:date ;
    dct:source "ISO/IEC 22989:2022"@en ;
    rdfs:isDefinedBy ai: ;
    sw:term_status "accepted"@en ;
    skos:broader ai:OperationStage ;
    skos:definition "The stage in the lifecycle where an AI system is actively being monitored for incidents"@en ;
    skos:inScheme ai:lifecycle-classes ;
    skos:prefLabel "Incident Monitoring Stage"@en .

ai:LifecycleStage a rdfs:Class,
        skos:Concept ;
    dct:contributor _:person-delaram-golpayegani ;
    dct:created "2024-12-01"^^xsd:date ;
    rdfs:isDefinedBy ai: ;
    rdfs:subClassOf tech:LifecycleStage ;
    sw:term_status "accepted"@en ;
    skos:broader tech:LifecycleStage ;
    skos:definition "A stage in the lifecycle of AI"@en ;
    skos:inScheme ai:lifecycle-classes ;
    skos:prefLabel "Lifecycle Stage"@en .

ai:OperationStage a rdfs:Class,
        skos:Concept,
        ai:LifecycleStage ;
    dct:contributor _:person-delaram-golpayegani ;
    dct:created "2024-12-01"^^xsd:date ;
    dct:source "ISO/IEC 22989:2022"@en ;
    rdfs:isDefinedBy ai: ;
    sw:term_status "accepted"@en ;
    skos:broader ai:LifecycleStage ;
    skos:definition "The stage in the lifecycle where an AI system is running and generally available for operations"@en ;
    skos:inScheme ai:lifecycle-classes ;
    skos:prefLabel "Operation Stage"@en .

ai:ReevaluationStage a rdfs:Class,
        skos:Concept,
        ai:LifecycleStage ;
    dct:contributor _:person-delaram-golpayegani ;
    dct:created "2024-12-01"^^xsd:date ;
    dct:source "ISO/IEC 22989:2022"@en ;
    rdfs:isDefinedBy ai: ;
    sw:term_status "accepted"@en ;
    skos:broader ai:LifecycleStage ;
    skos:definition "The stage in the lifecycle where the AI system is reevaluated after the operation and monitoring stage based on the operations of the AI system"@en ;
    skos:inScheme ai:lifecycle-classes ;
    skos:prefLabel "Reevaluation Stage"@en .

ai:RepairStage a rdfs:Class,
        skos:Concept,
        ai:LifecycleStage ;
    dct:contributor _:person-harshvardhan-j-pandit ;
    dct:created "2024-12-01"^^xsd:date ;
    dct:source "ISO/IEC 22989:2022"@en ;
    rdfs:isDefinedBy ai: ;
    sw:term_status "accepted"@en ;
    skos:broader ai:OperationStage ;
    skos:definition "The stage in the lifecycle where an AI system is being repaired due to suspected or occurred incidents"@en ;
    skos:inScheme ai:lifecycle-classes ;
    skos:prefLabel "Repair Stage"@en .

ai:ReplaceStage a rdfs:Class,
        skos:Concept,
        ai:LifecycleStage ;
    dct:contributor _:person-harshvardhan-j-pandit ;
    dct:created "2024-12-01"^^xsd:date ;
    dct:source "ISO/IEC 22989:2022"@en ;
    rdfs:isDefinedBy ai: ;
    sw:term_status "accepted"@en ;
    skos:broader ai:RetirementStage ;
    skos:definition "The stage in the lifecycle where the AI system is being replaced as part of retirement"@en ;
    skos:inScheme ai:lifecycle-classes ;
    skos:prefLabel "Replace Stage"@en .

ai:RetirementStage a rdfs:Class,
        skos:Concept,
        ai:LifecycleStage ;
    dct:contributor _:person-delaram-golpayegani ;
    dct:created "2024-12-01"^^xsd:date ;
    dct:source "ISO/IEC 22989:2022"@en ;
    rdfs:isDefinedBy ai: ;
    sw:term_status "accepted"@en ;
    skos:broader ai:LifecycleStage ;
    skos:definition "The stage in the lifecycle where the AI system is retired and becomes obsolete"@en ;
    skos:inScheme ai:lifecycle-classes ;
    skos:prefLabel "Retirement Stage"@en .

ai:UpdateStage a rdfs:Class,
        skos:Concept,
        ai:LifecycleStage ;
    dct:contributor _:person-harshvardhan-j-pandit ;
    dct:created "2024-12-01"^^xsd:date ;
    dct:source "ISO/IEC 22989:2022"@en ;
    rdfs:isDefinedBy ai: ;
    sw:term_status "accepted"@en ;
    skos:broader ai:OperationStage ;
    skos:definition "The stage in the lifecycle where an AI system is being or has been updated"@en ;
    skos:inScheme ai:lifecycle-classes ;
    skos:prefLabel "Update Stage"@en .

ai:ValidationStage a rdfs:Class,
        skos:Concept,
        ai:LifecycleStage ;
    dct:contributor _:person-delaram-golpayegani ;
    dct:created "2024-12-01"^^xsd:date ;
    dct:source "ISO/IEC 22989:2022"@en ;
    rdfs:isDefinedBy ai: ;
    sw:term_status "accepted"@en ;
    skos:broader ai:LifecycleStage ;
    skos:definition "The stage in the lifecycle where the AI system is validated for requirements and objectives for an intended use or application"@en ;
    skos:inScheme ai:lifecycle-classes ;
    skos:prefLabel "Validation Stage"@en .

ai:VerificationStage a rdfs:Class,
        skos:Concept,
        ai:LifecycleStage ;
    dct:contributor _:person-delaram-golpayegani ;
    dct:created "2024-12-01"^^xsd:date ;
    dct:source "ISO/IEC 22989:2022"@en ;
    rdfs:isDefinedBy ai: ;
    sw:term_status "accepted"@en ;
    skos:broader ai:LifecycleStage ;
    skos:definition "The stage in the lifecycle where the AI system is being verified to satisfy requirements and meet objectives"@en ;
    skos:inScheme ai:lifecycle-classes ;
    skos:prefLabel "Verification Stage"@en .

<https://w3id.org/dpv/ai> a owl:Ontology,
        profile:Profile ;
    dct:bibliographicCitation "Harshvardhan J. Pandit, Beatriz Esteves, Georg P. Krog, Paul Ryan, Delaram Golpayegani, Julian Flake (2025) Data Privacy Vocabulary (DPV) – Version 2.0. In: Demartini, G., et al. The Semantic Web – ISWC 2024. ISWC 2024. Lecture Notes in Computer Science, vol 15233. Springer, Cham. https://doi.org/10.1007/978-3-031-77847-6_10" ;
    dct:conformsTo "http://www.w3.org/2000/01/rdf-schema",
        "http://www.w3.org/2004/02/skos/core" ;
    dct:contributor _:person-arthit-suriyawongkul,
        _:person-delaram-golpayegani,
        _:person-harshvardhan-j-pandit ;
    dct:created "2024-05-31"@en ;
    dct:creator _:person-delaram-golpayegani,
        _:person-harshvardhan-j-pandit ;
    dct:description "Extension to the Data Privacy Vocabulary (DPV) providing concepts for representing information about AI technologies"@en ;
    dct:identifier "https://w3id.org/dpv/ai" ;
    dct:issued "2024-05-31"@en ;
    dct:license <https://www.w3.org/copyright/document-license-2023/> ;
    dct:modified "2025-08-01"@en ;
    dct:publisher <https://www.w3.org/> ;
    dct:source <https://www.w3.org/groups/cg/dpvcg/> ;
    dct:title "AI Technology Concepts"@en ;
    bibo:doi "10.5281/zenodo.12505841" ;
    bibo:status "http://purl.org/ontology/bibo/status/published" ;
    vann:preferredNamespacePrefix "ai" ;
    vann:preferredNamespaceUri "https://w3id.org/dpv/ai#" ;
    rdfs:Label "AI"@en ;
    owl:versionIRI <https://w3id.org/dpv/2.2/ai> ;
    owl:versionInfo "2.2" ;
    profile:hasResource ai:serialisation-html,
        ai:serialisation-ttl,
        <https://w3id.org/dpv/examples>,
        <https://w3id.org/dpv/guides>,
        <https://w3id.org/dpv/primer> ;
    profile:isProfileOf rdfs:,
        skos:,
        <https://w3id.org/dpv/tech> ;
    foaf:logo <https://w3id.org/dpv/media/logo.png> ;
    schema:version "2.2" .

ai:serialisation-html a profile:ResourceDescriptor ;
    dct:conformsTo <https://www.w3.org/TR/html/> ;
    dct:format <https://www.iana.org/assignments/media-types/text/html> ;
    dct:title "AI Technology Concepts - HTML serialisation" ;
    profile:hasArtifact <https://w3id.org/dpv/ai/ai.html> ;
    profile:hasRole role:specification .

ai:serialisation-ttl a profile:ResourceDescriptor ;
    dct:conformsTo <https://www.w3.org/TR/turtle/> ;
    dct:format <https://www.iana.org/assignments/media-types/text/turtle> ;
    dct:title "AI Technology Concepts - Turtle serialisation" ;
    profile:hasArtifact <https://w3id.org/dpv/ai/ai.ttl> ;
    profile:hasRole role:vocabulary .

<https://w3id.org/dpv/examples> a profile:ResourceDescriptor ;
    dct:conformsTo <https://www.w3.org/TR/html/> ;
    dct:format <https://www.iana.org/assignments/media-types/text/html> ;
    dct:title "Examples" ;
    profile:hasArtifact <https://w3id.org/dpv/examples> ;
    profile:hasRole role:guidance .

<https://w3id.org/dpv/guides> a profile:ResourceDescriptor ;
    dct:conformsTo <https://www.w3.org/TR/html/> ;
    dct:format <https://www.iana.org/assignments/media-types/text/html> ;
    dct:title "Guides for Data Privacy Vocabulary" ;
    profile:hasArtifact <https://w3id.org/dpv/guides> ;
    profile:hasRole role:guidance .

<https://w3id.org/dpv/primer> a profile:ResourceDescriptor ;
    dct:conformsTo <https://www.w3.org/TR/html/> ;
    dct:format <https://www.iana.org/assignments/media-types/text/html> ;
    dct:title "Primer for Data Privacy Vocabulary" ;
    profile:hasArtifact <https://w3id.org/dpv/primer> ;
    profile:hasRole role:guidance .

ai:lifecycle-classes a skos:ConceptScheme .

_:org-ai-accountability-lab-aial-trinity-college-dublin a foaf:Organization ;
    foaf:name "AI Accountability Lab (AIAL), Trinity College Dublin" .

_:org-adapt-centre-trinity-college-dublin a foaf:Organization ;
    foaf:name "ADAPT Centre, Trinity College Dublin" .

_:person-arthit-suriyawongkul a dct:Agent,
        foaf:Person ;
    scoro:hasORCID "0000-0002-9698-1899" ;
    org:memberOf _:org-adapt-centre-trinity-college-dublin ;
    foaf:name "Arthit Suriyawongkul" .

_:person-harshvardhan-j-pandit a dct:Agent,
        foaf:Person ;
    scoro:hasORCID "0000-0002-5068-3714" ;
    org:memberOf _:org-ai-accountability-lab-aial-trinity-college-dublin ;
    foaf:homepage "https://harshp.com/" ;
    foaf:name "Harshvardhan J. Pandit" .

_:person-delaram-golpayegani a dct:Agent,
        foaf:Person ;
    scoro:hasORCID "0000-0002-1208-186X" ;
    org:memberOf _:org-adapt-centre-trinity-college-dublin ;
    foaf:name "Delaram Golpayegani" .

