@prefix bibo: <http://purl.org/ontology/bibo/> .
@prefix dct: <http://purl.org/dc/terms/> .
@prefix dpv: <https://w3id.org/dpv#> .
@prefix eu-ehds: <https://w3id.org/dpv/legal/eu/ehds#> .
@prefix foaf: <http://xmlns.com/foaf/0.1/> .
@prefix org: <http://www.w3.org/ns/org#> .
@prefix owl: <http://www.w3.org/2002/07/owl#> .
@prefix profile: <http://www.w3.org/ns/dx/prof/> .
@prefix rdfs: <http://www.w3.org/2000/01/rdf-schema#> .
@prefix role: <http://www.w3.org/ns/dx/prof/role/> .
@prefix schema: <https://schema.org/> .
@prefix scoro: <http://purl.org/spar/scoro/> .
@prefix sector-health: <https://w3id.org/dpv/sector/health#> .
@prefix skos: <http://www.w3.org/2004/02/skos/core#> .
@prefix sw: <http://www.w3.org/2003/06/sw-vocab-status/ns#> .
@prefix vann: <http://purl.org/vocab/vann/> .
@prefix xsd: <http://www.w3.org/2001/XMLSchema#> .

eu-ehds:AdministrativeServicesProvision a rdfs:Class,
        skos:Concept,
        dpv:Purpose ;
    dct:contributor _:person-beatriz-esteves ;
    dct:created "2025-10-28"^^xsd:date ;
    dct:source "EHDS Art.2.2(d)"@en ;
    rdfs:isDefinedBy eu-ehds: ;
    sw:term_status "accepted"@en ;
    skos:broader sector-health:AdministrativeServicesProvision ;
    skos:definition "Purposes associated with the provision of administrative services related to healthcare"@en ;
    skos:inScheme eu-ehds:purposes-classes ;
    skos:prefLabel "Administrative Services Provision"@en .

eu-ehds:DevelopPublicHealthProductsAndServices a rdfs:Class,
        skos:Concept,
        dpv:Purpose ;
    dct:contributor _:person-beatriz-esteves ;
    dct:created "2024-12-01"^^xsd:date ;
    dct:modified "2026-02-04"^^xsd:date ;
    dct:source "EHDS Art.53.1(e)(i)"@en ;
    rdfs:isDefinedBy eu-ehds: ;
    sw:term_status "modified"@en ;
    skos:broader sector-health:DevelopPublicHealthProductsAndServices ;
    skos:definition "Purposes associated with developing products and services that contribute to public health"@en ;
    skos:inScheme eu-ehds:purposes-classes ;
    skos:prefLabel "Develop Public Health Products and Services"@en .

eu-ehds:EnsureQualitySafetyHealthcare a rdfs:Class,
        skos:Concept,
        dpv:Purpose ;
    dct:contributor _:person-beatriz-esteves ;
    dct:created "2024-12-01"^^xsd:date ;
    dct:modified "2026-02-04"^^xsd:date ;
    dct:source "EHDS Art.53.1(a)"@en ;
    rdfs:isDefinedBy eu-ehds: ;
    sw:term_status "modified"@en ;
    skos:broader sector-health:EnsureQualitySafetyHealthcare ;
    skos:definition "Purposes associated with ensuring high levels of quality and safety of healthcare, including patients safety"@en ;
    skos:inScheme eu-ehds:purposes-classes ;
    skos:prefLabel "Ensure Quality and Safety of Healthcare"@en .

eu-ehds:EnsureQualitySafetyMedicalDevices a rdfs:Class,
        skos:Concept,
        dpv:Purpose ;
    dct:contributor _:person-beatriz-esteves ;
    dct:created "2024-12-01"^^xsd:date ;
    dct:modified "2026-02-04"^^xsd:date ;
    dct:source "EHDS Art.53.1(a)"@en ;
    rdfs:isDefinedBy eu-ehds: ;
    sw:term_status "modified"@en ;
    skos:broader sector-health:EnsureQualitySafetyMedicalDevices ;
    skos:definition "Purposes associated with ensuring high levels of quality and safety of medical devices"@en ;
    skos:inScheme eu-ehds:purposes-classes ;
    skos:prefLabel "Ensure Quality and Safety of Medical Devices"@en .

eu-ehds:EnsureQualitySafetyMedicinalProducts a rdfs:Class,
        skos:Concept,
        dpv:Purpose ;
    dct:contributor _:person-beatriz-esteves ;
    dct:created "2024-12-01"^^xsd:date ;
    dct:modified "2026-02-04"^^xsd:date ;
    dct:source "EHDS Art.53.1(a)"@en ;
    rdfs:isDefinedBy eu-ehds: ;
    sw:term_status "modified"@en ;
    skos:broader sector-health:EnsureQualitySafetyMedicinalProducts ;
    skos:definition "Purposes associated with ensuring high levels of quality and safety of medicinal products"@en ;
    skos:inScheme eu-ehds:purposes-classes ;
    skos:prefLabel "Ensure Quality and Safety of Medicinal Products"@en .

eu-ehds:HealthcareScientificResearch a rdfs:Class,
        skos:Concept,
        dpv:Purpose ;
    dct:contributor _:person-beatriz-esteves ;
    dct:created "2024-12-01"^^xsd:date ;
    dct:modified "2026-02-04"^^xsd:date ;
    dct:source "EHDS Art.53.1(e)"@en ;
    rdfs:isDefinedBy eu-ehds: ;
    sw:term_status "modified"@en ;
    skos:broader sector-health:HealthcareScientificResearch ;
    skos:definition "Purposes associated with healthcare scientific research"@en ;
    skos:inScheme eu-ehds:purposes-classes ;
    skos:prefLabel "Healthcare Scientific Research"@en .

eu-ehds:ImproveHealthcare a rdfs:Class,
        skos:Concept,
        dpv:Purpose ;
    dct:contributor _:person-beatriz-esteves ;
    dct:created "2026-02-04"^^xsd:date ;
    dct:source "EHDS Art.53.1(f)"@en ;
    rdfs:isDefinedBy eu-ehds: ;
    sw:term_status "accepted"@en ;
    skos:broader sector-health:ImproveHealthcare ;
    skos:definition "Purposes associated with improving healthcare systems, including the delivery of care and the provision and optimisation of treatment"@en ;
    skos:inScheme eu-ehds:purposes-classes ;
    skos:prefLabel "Improve Healthcare"@en .

eu-ehds:ImproveHealthcareEducation a rdfs:Class,
        skos:Concept,
        dpv:Purpose ;
    dct:contributor _:person-beatriz-esteves ;
    dct:created "2024-12-01"^^xsd:date ;
    dct:modified "2026-02-04"^^xsd:date ;
    dct:source "EHDS Art.53.1(d)"@en ;
    rdfs:isDefinedBy eu-ehds: ;
    sw:term_status "modified"@en ;
    skos:broader sector-health:ImproveHealthcareEducation ;
    skos:definition "Purposes associated with improving the provision of healthcare education"@en ;
    skos:inScheme eu-ehds:purposes-classes ;
    skos:prefLabel "Improve Healthcare Education"@en .

eu-ehds:MedicalDevicesDispensation a rdfs:Class,
        skos:Concept,
        dpv:Purpose ;
    dct:contributor _:person-beatriz-esteves ;
    dct:created "2025-10-28"^^xsd:date ;
    dct:source "EHDS Art.2.2(d)"@en ;
    rdfs:isDefinedBy eu-ehds: ;
    sw:term_status "accepted"@en ;
    skos:broader sector-health:MedicalDevicesDispensation ;
    skos:definition "Purposes associated with the dispensation of medical devices"@en ;
    skos:inScheme eu-ehds:purposes-classes ;
    skos:prefLabel "Medical Devices Dispensation"@en .

eu-ehds:MedicalDevicesPrescription a rdfs:Class,
        skos:Concept,
        dpv:Purpose ;
    dct:contributor _:person-beatriz-esteves ;
    dct:created "2025-10-28"^^xsd:date ;
    dct:source "EHDS Art.2.2(d)"@en ;
    rdfs:isDefinedBy eu-ehds: ;
    sw:term_status "accepted"@en ;
    skos:broader sector-health:MedicalDevicesPrescription ;
    skos:definition "Purposes associated with prescription of medical devices"@en ;
    skos:inScheme eu-ehds:purposes-classes ;
    skos:prefLabel "Medical Devices Prescription"@en .

eu-ehds:MedicalDevicesProvision a rdfs:Class,
        skos:Concept,
        dpv:Purpose ;
    dct:contributor _:person-beatriz-esteves ;
    dct:created "2025-10-28"^^xsd:date ;
    dct:source "EHDS Art.2.2(d)"@en ;
    rdfs:isDefinedBy eu-ehds: ;
    sw:term_status "accepted"@en ;
    skos:broader sector-health:MedicalDevicesProvision ;
    skos:definition "Purposes associated with the provision of medical devices"@en ;
    skos:inScheme eu-ehds:purposes-classes ;
    skos:prefLabel "Medical Devices Provision"@en .

eu-ehds:MedicinalProductsDispensation a rdfs:Class,
        skos:Concept,
        dpv:Purpose ;
    dct:contributor _:person-beatriz-esteves ;
    dct:created "2025-10-28"^^xsd:date ;
    dct:source "EHDS Art.2.2(d)"@en ;
    rdfs:isDefinedBy eu-ehds: ;
    sw:term_status "accepted"@en ;
    skos:broader sector-health:MedicinalProductsDispensation ;
    skos:definition "Purposes associated with the dispensation of medicinal products"@en ;
    skos:inScheme eu-ehds:purposes-classes ;
    skos:prefLabel "Medicinal Products Dispensation"@en .

eu-ehds:MedicinalProductsPrescription a rdfs:Class,
        skos:Concept,
        dpv:Purpose ;
    dct:contributor _:person-beatriz-esteves ;
    dct:created "2025-10-28"^^xsd:date ;
    dct:source "EHDS Art.2.2(d)"@en ;
    rdfs:isDefinedBy eu-ehds: ;
    sw:term_status "accepted"@en ;
    skos:broader sector-health:MedicinalProductsPrescription ;
    skos:definition "Purposes associated with prescription of medicinal products"@en ;
    skos:inScheme eu-ehds:purposes-classes ;
    skos:prefLabel "Medicinal Products Prescription"@en .

eu-ehds:MedicinalProductsProvision a rdfs:Class,
        skos:Concept,
        dpv:Purpose ;
    dct:contributor _:person-beatriz-esteves ;
    dct:created "2025-10-28"^^xsd:date ;
    dct:source "EHDS Art.2.2(d)"@en ;
    rdfs:isDefinedBy eu-ehds: ;
    sw:term_status "accepted"@en ;
    skos:broader sector-health:MedicinalProductsProvision ;
    skos:definition "Purposes associated with the provision of medicinal products"@en ;
    skos:inScheme eu-ehds:purposes-classes ;
    skos:prefLabel "Medicinal Products Provision"@en .

eu-ehds:ProtectAgainstCrossBorderThreatsToHealth a rdfs:Class,
        skos:Concept,
        dpv:Purpose ;
    dct:contributor _:person-beatriz-esteves ;
    dct:created "2024-12-01"^^xsd:date ;
    dct:modified "2026-02-04"^^xsd:date ;
    dct:source "EHDS Art.53.1(a)"@en ;
    rdfs:isDefinedBy eu-ehds: ;
    sw:term_status "modified"@en ;
    skos:broader sector-health:ProtectAgainstCrossBorderThreatsToHealth ;
    skos:definition "Purposes associated with the protection against serious cross-border threats to health"@en ;
    skos:inScheme eu-ehds:purposes-classes ;
    skos:prefLabel "Protect against Cross-border Threats to Health"@en .

eu-ehds:ProvideHealthcareOfficialStatistics a rdfs:Class,
        skos:Concept,
        dpv:Purpose ;
    dct:contributor _:person-beatriz-esteves ;
    dct:created "2024-12-01"^^xsd:date ;
    dct:modified "2026-02-04"^^xsd:date ;
    dct:source "EHDS Art.53.1(c)"@en ;
    rdfs:isDefinedBy eu-ehds: ;
    sw:term_status "modified"@en ;
    skos:broader sector-health:ProvideHealthcareOfficialStatistics ;
    skos:definition "Purposes associated with facilitating the development, production and dissemination of reliable official statistics related to health or care sectors"@en ;
    skos:inScheme eu-ehds:purposes-classes ;
    skos:prefLabel "Provide Healthcare Official Statistics"@en .

eu-ehds:PublicHealthSurveillance a rdfs:Class,
        skos:Concept,
        dpv:Purpose ;
    dct:contributor _:person-beatriz-esteves ;
    dct:created "2024-12-01"^^xsd:date ;
    dct:modified "2026-02-04"^^xsd:date ;
    dct:source "EHDS Art.53.1(a)"@en ;
    rdfs:isDefinedBy eu-ehds: ;
    sw:term_status "modified"@en ;
    skos:broader sector-health:PublicHealthSurveillance ;
    skos:definition "Purposes associated with public health surveillance"@en ;
    skos:inScheme eu-ehds:purposes-classes ;
    skos:prefLabel "Public Health Surveillance"@en .

eu-ehds:PublicInterestRelatedToHealth a rdfs:Class,
        skos:Concept,
        dpv:Purpose ;
    dct:contributor _:person-beatriz-esteves ;
    dct:created "2024-12-01"^^xsd:date ;
    dct:modified "2026-02-04"^^xsd:date ;
    dct:source "EHDS Art.53.1(a)"@en ;
    rdfs:isDefinedBy eu-ehds: ;
    sw:term_status "modified"@en ;
    skos:broader sector-health:PublicInterestRelatedToHealth ;
    skos:definition "Purposes associated with pursuing activities for reasons of public interest in the area of public and occupational health"@en ;
    skos:inScheme eu-ehds:purposes-classes ;
    skos:prefLabel "Public Interest related to Health"@en .

eu-ehds:PublicPolicyMaking a rdfs:Class,
        skos:Concept,
        dpv:Purpose ;
    dct:contributor _:person-beatriz-esteves ;
    dct:created "2026-02-04"^^xsd:date ;
    dct:source "EHDS Art.53.1(b)"@en ;
    rdfs:isDefinedBy eu-ehds: ;
    sw:term_status "accepted"@en ;
    skos:broader sector-health:PublicPolicyMaking ;
    skos:definition "Purposes associated with public policy making policymaking in the healthcare sector"@en ;
    skos:inScheme eu-ehds:purposes-classes ;
    skos:prefLabel "Public Policy Making"@en .

eu-ehds:ReimbursementServicesProvision a rdfs:Class,
        skos:Concept,
        dpv:Purpose ;
    dct:contributor _:person-beatriz-esteves ;
    dct:created "2025-10-28"^^xsd:date ;
    dct:source "EHDS Art.2.2(d)"@en ;
    rdfs:isDefinedBy eu-ehds: ;
    sw:term_status "accepted"@en ;
    skos:broader sector-health:ReimbursementServicesProvision ;
    skos:definition "Purposes associated with the provision of reimbursement services related to healthcare"@en ;
    skos:inScheme eu-ehds:purposes-classes ;
    skos:prefLabel "Reimbursement Services Provision"@en .

eu-ehds:SocialServicesProvision a rdfs:Class,
        skos:Concept,
        dpv:Purpose ;
    dct:contributor _:person-beatriz-esteves ;
    dct:created "2025-10-28"^^xsd:date ;
    dct:source "EHDS Art.2.2(d)"@en ;
    rdfs:isDefinedBy eu-ehds: ;
    sw:term_status "accepted"@en ;
    skos:broader sector-health:SocialServicesProvision ;
    skos:definition "Purposes associated with the provision of social services related to healthcare"@en ;
    skos:inScheme eu-ehds:purposes-classes ;
    skos:prefLabel "Social Services Provision"@en .

eu-ehds:SupportAuthoritiesRegulatoryActivities a rdfs:Class,
        skos:Concept,
        dpv:Purpose ;
    dct:contributor _:person-beatriz-esteves ;
    dct:created "2024-12-01"^^xsd:date ;
    dct:modified "2026-02-04"^^xsd:date ;
    dct:source "EHDS Art.53.1(b)"@en ;
    rdfs:isDefinedBy eu-ehds: ;
    sw:term_status "modified"@en ;
    skos:broader sector-health:SupportAuthoritiesRegulatoryActivities ;
    skos:definition "Purposes associated with supporting authorities to carry out their regulatory tasks"@en ;
    skos:inScheme eu-ehds:purposes-classes ;
    skos:prefLabel "Support Authorities in Regulatory Activities"@en .

eu-ehds:TrainTestAndEvaluateAISystemsAlgorithms a rdfs:Class,
        skos:Concept,
        dpv:Purpose ;
    dct:contributor _:person-beatriz-esteves ;
    dct:created "2024-12-01"^^xsd:date ;
    dct:modified "2026-02-04"^^xsd:date ;
    dct:source "EHDS Art.53.1(e)(ii)"@en ;
    rdfs:isDefinedBy eu-ehds: ;
    sw:term_status "modified"@en ;
    skos:broader sector-health:TrainTestAndEvaluateAISystemsAlgorithms ;
    skos:definition "Purposes associated with training, testing and evaluating algorithms in AI systems"@en ;
    skos:inScheme eu-ehds:purposes-classes ;
    skos:prefLabel "Train, Test and Evaluate AI Systems Algorithms"@en .

eu-ehds:TrainTestAndEvaluateHealthAlgorithms a rdfs:Class,
        skos:Concept,
        dpv:Purpose ;
    dct:contributor _:person-beatriz-esteves ;
    dct:created "2024-12-01"^^xsd:date ;
    dct:modified "2026-02-04"^^xsd:date ;
    dct:source "EHDS Art.53.1(e)(ii)"@en ;
    rdfs:isDefinedBy eu-ehds: ;
    sw:term_status "modified"@en ;
    skos:broader sector-health:TrainTestAndEvaluateHealthAlgorithms ;
    skos:definition "Purposes associated with training, testing and evaluating health-related algorithms"@en ;
    skos:inScheme eu-ehds:purposes-classes ;
    skos:prefLabel "Train, Test and Evaluate Health-related Algorithms"@en .

eu-ehds:TrainTestAndEvaluateHealthAppsAlgorithms a rdfs:Class,
        skos:Concept,
        dpv:Purpose ;
    dct:contributor _:person-beatriz-esteves ;
    dct:created "2024-12-01"^^xsd:date ;
    dct:modified "2026-02-04"^^xsd:date ;
    dct:source "EHDS Art.53.1(e)(ii)"@en ;
    rdfs:isDefinedBy eu-ehds: ;
    sw:term_status "modified"@en ;
    skos:broader sector-health:TrainTestAndEvaluateHealthAppsAlgorithms ;
    skos:definition "Purposes associated with training, testing and evaluating algorithms in digital health applications"@en ;
    skos:inScheme eu-ehds:purposes-classes ;
    skos:prefLabel "Train, Test and Evaluate Health Apps Algorithms"@en .

eu-ehds:TrainTestAndEvaluateMedicalDevicesAlgorithms a rdfs:Class,
        skos:Concept,
        dpv:Purpose ;
    dct:contributor _:person-beatriz-esteves ;
    dct:created "2024-12-01"^^xsd:date ;
    dct:modified "2026-02-04"^^xsd:date ;
    dct:source "EHDS Art.53.1(e)(ii)"@en ;
    rdfs:isDefinedBy eu-ehds: ;
    sw:term_status "modified"@en ;
    skos:broader sector-health:TrainTestAndEvaluateMedicalDevicesAlgorithms ;
    skos:definition "Purposes associated with training, testing and evaluating algorithms in medical devices"@en ;
    skos:inScheme eu-ehds:purposes-classes ;
    skos:prefLabel "Train, Test and Evaluate Medical Devices Algorithms"@en .

<https://w3id.org/dpv/legal/eu/ehds> a owl:Ontology,
        profile:Profile ;
    dct:bibliographicCitation "Harshvardhan J. Pandit, Beatriz Esteves, Georg P. Krog, Paul Ryan, Delaram Golpayegani, Julian Flake (2025) Data Privacy Vocabulary (DPV) – Version 2.0. In: Demartini, G., et al. The Semantic Web – ISWC 2024. ISWC 2024. Lecture Notes in Computer Science, vol 15233. Springer, Cham. https://doi.org/10.1007/978-3-031-77847-6_10" ;
    dct:conformsTo "http://www.w3.org/2000/01/rdf-schema",
        "http://www.w3.org/2004/02/skos/core" ;
    dct:contributor _:person-beatriz-esteves ;
    dct:created "2024-12-01"@en ;
    dct:creator _:person-beatriz-esteves,
        [ a dct:Agent,
                foaf:Person ;
            scoro:hasORCID "0000-0002-5068-3714" ;
            org:memberOf [ a foaf:Organization ;
                    foaf:name "AI Accountability Lab (AIAL), Trinity College Dublin" ] ;
            foaf:homepage "https://harshp.com/" ;
            foaf:name "Harshvardhan J. Pandit" ] ;
    dct:description "Extension to the Data Privacy Vocabulary (DPV) providing concepts for representing information associated with EU Health Data Spaces (EHDS)"@en ;
    dct:identifier "https://w3id.org/dpv/legal/eu/ehds" ;
    dct:issued "2024-12-01"@en ;
    dct:license <https://www.w3.org/copyright/document-license-2023/> ;
    dct:modified "2026-02-25"@en ;
    dct:publisher <https://www.w3.org/> ;
    dct:source <https://www.w3.org/groups/cg/dpvcg/> ;
    dct:title "EU European Health Data Spaces (EHDS)"@en ;
    bibo:doi "10.5281/zenodo.12505841" ;
    bibo:status "http://purl.org/ontology/bibo/status/draft" ;
    vann:preferredNamespacePrefix "eu-ehds" ;
    vann:preferredNamespaceUri "https://w3id.org/dpv/legal/eu/ehds#" ;
    rdfs:Label "EU-EHDS"@en ;
    owl:versionIRI <https://w3id.org/dpv/2.3/legal/eu/ehds> ;
    owl:versionInfo "2.3" ;
    profile:hasResource <https://w3id.org/dpv/examples>,
        <https://w3id.org/dpv/guides>,
        eu-ehds:serialisation-html,
        eu-ehds:serialisation-ttl,
        <https://w3id.org/dpv/primer> ;
    profile:isProfileOf rdfs:,
        skos:,
        <https://w3id.org/dpv> ;
    foaf:logo <https://w3id.org/dpv/media/logo.png> ;
    schema:version "2.3" .

eu-ehds:serialisation-html a profile:ResourceDescriptor ;
    dct:conformsTo <https://www.w3.org/TR/html/> ;
    dct:format <https://www.iana.org/assignments/media-types/text/html> ;
    dct:title "EU European Health Data Spaces (EHDS) - HTML serialisation" ;
    profile:hasArtifact <https://w3id.org/dpv/legal/eu/ehds/eu-ehds.html> ;
    profile:hasRole role:specification .

eu-ehds:serialisation-ttl a profile:ResourceDescriptor ;
    dct:conformsTo <https://www.w3.org/TR/turtle/> ;
    dct:format <https://www.iana.org/assignments/media-types/text/turtle> ;
    dct:title "EU European Health Data Spaces (EHDS) - Turtle serialisation" ;
    profile:hasArtifact <https://w3id.org/dpv/legal/eu/ehds/eu-ehds.ttl> ;
    profile:hasRole role:vocabulary .

<https://w3id.org/dpv/examples> a profile:ResourceDescriptor ;
    dct:conformsTo <https://www.w3.org/TR/html/> ;
    dct:format <https://www.iana.org/assignments/media-types/text/html> ;
    dct:title "Examples" ;
    profile:hasArtifact <https://w3id.org/dpv/examples> ;
    profile:hasRole role:guidance .

<https://w3id.org/dpv/guides> a profile:ResourceDescriptor ;
    dct:conformsTo <https://www.w3.org/TR/html/> ;
    dct:format <https://www.iana.org/assignments/media-types/text/html> ;
    dct:title "Guides for Data Privacy Vocabulary" ;
    profile:hasArtifact <https://w3id.org/dpv/guides> ;
    profile:hasRole role:guidance .

<https://w3id.org/dpv/primer> a profile:ResourceDescriptor ;
    dct:conformsTo <https://www.w3.org/TR/html/> ;
    dct:format <https://www.iana.org/assignments/media-types/text/html> ;
    dct:title "Primer for Data Privacy Vocabulary" ;
    profile:hasArtifact <https://w3id.org/dpv/primer> ;
    profile:hasRole role:guidance .

eu-ehds:purposes-classes a skos:ConceptScheme .

_:org-idlab-imec-ghent-university a foaf:Organization ;
    foaf:name "IDLab, IMEC, Ghent University" .

_:person-beatriz-esteves a dct:Agent,
        foaf:Person ;
    scoro:hasORCID "0000-0003-0259-7560" ;
    org:memberOf _:org-idlab-imec-ghent-university ;
    foaf:homepage "https://w3id.org/people/besteves" ;
    foaf:name "Beatriz Esteves" .

