<?xml version="1.0" encoding="utf-8"?>
<rdf:RDF
   xmlns:bibo="http://purl.org/ontology/bibo/"
   xmlns:dct="http://purl.org/dc/terms/"
   xmlns:foaf="http://xmlns.com/foaf/0.1/"
   xmlns:org="http://www.w3.org/ns/org#"
   xmlns:owl="http://www.w3.org/2002/07/owl#"
   xmlns:profile="http://www.w3.org/ns/dx/prof/"
   xmlns:rdf="http://www.w3.org/1999/02/22-rdf-syntax-ns#"
   xmlns:rdfs="http://www.w3.org/2000/01/rdf-schema#"
   xmlns:schema="https://schema.org/"
   xmlns:scoro="http://purl.org/spar/scoro/"
   xmlns:skos="http://www.w3.org/2004/02/skos/core#"
   xmlns:sw="http://www.w3.org/2003/06/sw-vocab-status/ns#"
   xmlns:vann="http://purl.org/vocab/vann/"
>
  <rdf:Description rdf:about="https://w3id.org/dpv/legal/eu/ehds#A16-1">
    <rdf:type rdf:resource="http://www.w3.org/2004/02/skos/core#Concept"/>
    <rdf:type rdf:resource="http://www.w3.org/2000/01/rdf-schema#Class"/>
    <rdf:type rdf:resource="https://w3id.org/dpv#Right"/>
    <skos:prefLabel xml:lang="en">A16-1 Right of identification management</skos:prefLabel>
    <skos:definition xml:lang="en">Right of natural persons to identify themselves electronically using any electronic identification means which are recognised pursuant to Article 6 of Regulation (EU) No 910/2014</skos:definition>
    <skos:broader rdf:resource="https://w3id.org/dpv#Right"/>
    <dct:source xml:lang="en">EHDS Art.16.1</dct:source>
    <dct:created rdf:datatype="http://www.w3.org/2001/XMLSchema#date">2025-10-28</dct:created>
    <sw:term_status xml:lang="en">accepted</sw:term_status>
    <dct:contributor rdf:nodeID="person-beatriz-esteves"/>
    <rdfs:isDefinedBy rdf:resource="https://w3id.org/dpv/legal/eu/ehds#"/>
    <skos:inScheme rdf:resource="https://w3id.org/dpv/legal/eu/ehds#rights-classes"/>
  </rdf:Description>
  <rdf:Description rdf:about="https://w3id.org/dpv/legal/eu/ehds#A68-11">
    <rdf:type rdf:resource="http://www.w3.org/2004/02/skos/core#Concept"/>
    <rdf:type rdf:resource="http://www.w3.org/2000/01/rdf-schema#Class"/>
    <rdf:type rdf:resource="https://w3id.org/dpv#Right"/>
    <skos:prefLabel xml:lang="en">A68-11 Right to process in a secure processing environment</skos:prefLabel>
    <skos:definition xml:lang="en">Right of health data users to access and process the electronic health data in a secure processing environment in accordance with the data permit issued to them</skos:definition>
    <skos:broader rdf:resource="https://w3id.org/dpv#Right"/>
    <dct:source xml:lang="en">EHDS Art.68.11</dct:source>
    <dct:created rdf:datatype="http://www.w3.org/2001/XMLSchema#date">2025-10-28</dct:created>
    <sw:term_status xml:lang="en">accepted</sw:term_status>
    <dct:contributor rdf:nodeID="person-beatriz-esteves"/>
    <rdfs:isDefinedBy rdf:resource="https://w3id.org/dpv/legal/eu/ehds#"/>
    <skos:inScheme rdf:resource="https://w3id.org/dpv/legal/eu/ehds#rights-classes"/>
  </rdf:Description>
  <rdf:Description rdf:about="https://w3id.org/dpv/legal/eu/ehds#A8">
    <rdf:type rdf:resource="http://www.w3.org/2004/02/skos/core#Concept"/>
    <rdf:type rdf:resource="http://www.w3.org/2000/01/rdf-schema#Class"/>
    <rdf:type rdf:resource="https://w3id.org/dpv#Right"/>
    <skos:prefLabel xml:lang="en">A8 Right to restrict access</skos:prefLabel>
    <skos:definition xml:lang="en">Right of natural persons to restrict the access of health professionals and healthcare providers to all or parts of their personal electronic health data</skos:definition>
    <skos:broader rdf:resource="https://w3id.org/dpv#Right"/>
    <dct:source xml:lang="en">EHDS Art.8</dct:source>
    <dct:created rdf:datatype="http://www.w3.org/2001/XMLSchema#date">2025-10-28</dct:created>
    <sw:term_status xml:lang="en">accepted</sw:term_status>
    <dct:contributor rdf:nodeID="person-beatriz-esteves"/>
    <rdfs:isDefinedBy rdf:resource="https://w3id.org/dpv/legal/eu/ehds#"/>
    <skos:inScheme rdf:resource="https://w3id.org/dpv/legal/eu/ehds#rights-classes"/>
  </rdf:Description>
  <rdf:Description rdf:about="https://w3id.org/dpv/legal/eu/ehds#A10">
    <rdf:type rdf:resource="http://www.w3.org/2004/02/skos/core#Concept"/>
    <rdf:type rdf:resource="http://www.w3.org/2000/01/rdf-schema#Class"/>
    <rdf:type rdf:resource="https://w3id.org/dpv#Right"/>
    <skos:prefLabel xml:lang="en">A10 Right of natural persons to opt out from primary use</skos:prefLabel>
    <skos:definition xml:lang="en">Right of natural persons to opt out from the access to their personal electronic health data registered in an EHR system through the electronic health data access services</skos:definition>
    <skos:broader rdf:resource="https://w3id.org/dpv#Right"/>
    <dct:source xml:lang="en">EHDS Art.10</dct:source>
    <dct:created rdf:datatype="http://www.w3.org/2001/XMLSchema#date">2025-10-28</dct:created>
    <sw:term_status xml:lang="en">accepted</sw:term_status>
    <dct:contributor rdf:nodeID="person-beatriz-esteves"/>
    <rdfs:isDefinedBy rdf:resource="https://w3id.org/dpv/legal/eu/ehds#"/>
    <skos:inScheme rdf:resource="https://w3id.org/dpv/legal/eu/ehds#rights-classes"/>
  </rdf:Description>
  <rdf:Description rdf:about="https://w3id.org/dpv/legal/eu/ehds#serialisation-html">
    <rdf:type rdf:resource="http://www.w3.org/ns/dx/prof/ResourceDescriptor"/>
    <profile:hasRole rdf:resource="http://www.w3.org/ns/dx/prof/role/specification"/>
    <profile:hasArtifact rdf:resource="https://w3id.org/dpv/legal/eu/ehds/eu-ehds.html"/>
    <dct:format rdf:resource="https://www.iana.org/assignments/media-types/text/html"/>
    <dct:conformsTo rdf:resource="https://www.w3.org/TR/html/"/>
    <dct:title>EU European Health Data Spaces (EHDS) - HTML serialisation</dct:title>
  </rdf:Description>
  <rdf:Description rdf:about="https://w3id.org/dpv/legal/eu/ehds#serialisation-ttl">
    <rdf:type rdf:resource="http://www.w3.org/ns/dx/prof/ResourceDescriptor"/>
    <profile:hasRole rdf:resource="http://www.w3.org/ns/dx/prof/role/vocabulary"/>
    <profile:hasArtifact rdf:resource="https://w3id.org/dpv/legal/eu/ehds/eu-ehds.ttl"/>
    <dct:format rdf:resource="https://www.iana.org/assignments/media-types/text/turtle"/>
    <dct:conformsTo rdf:resource="https://www.w3.org/TR/turtle/"/>
    <dct:title>EU European Health Data Spaces (EHDS) - Turtle serialisation</dct:title>
  </rdf:Description>
  <rdf:Description rdf:about="https://w3id.org/dpv/legal/eu/ehds">
    <rdf:type rdf:resource="http://www.w3.org/2002/07/owl#Ontology"/>
    <rdf:type rdf:resource="http://www.w3.org/ns/dx/prof/Profile"/>
    <owl:versionIRI rdf:resource="https://w3id.org/dpv/2.3/legal/eu/ehds"/>
    <dct:source rdf:resource="https://www.w3.org/groups/cg/dpvcg/"/>
    <dct:title xml:lang="en">EU European Health Data Spaces (EHDS)</dct:title>
    <bibo:status>http://purl.org/ontology/bibo/status/draft</bibo:status>
    <rdfs:Label xml:lang="en">EU-EHDS</rdfs:Label>
    <dct:description xml:lang="en">Extension to the Data Privacy Vocabulary (DPV) providing concepts for representing information associated with EU Health Data Spaces (EHDS)</dct:description>
    <dct:created xml:lang="en">2024-12-01</dct:created>
    <dct:issued xml:lang="en">2024-12-01</dct:issued>
    <dct:modified xml:lang="en">2026-02-25</dct:modified>
    <dct:creator rdf:nodeID="person-beatriz-esteves"/>
    <dct:creator rdf:nodeID="person-harshvardhan-j-pandit"/>
    <schema:version>2.3</schema:version>
    <owl:versionInfo>2.3</owl:versionInfo>
    <dct:identifier>https://w3id.org/dpv/legal/eu/ehds</dct:identifier>
    <dct:conformsTo>http://www.w3.org/2000/01/rdf-schema</dct:conformsTo>
    <dct:conformsTo>http://www.w3.org/2004/02/skos/core</dct:conformsTo>
    <bibo:doi>10.5281/zenodo.12505841</bibo:doi>
    <dct:bibliographicCitation>Harshvardhan J. Pandit, Beatriz Esteves, Georg P. Krog, Paul Ryan, Delaram Golpayegani, Julian Flake (2025) Data Privacy Vocabulary (DPV) – Version 2.0. In: Demartini, G., et al. The Semantic Web – ISWC 2024. ISWC 2024. Lecture Notes in Computer Science, vol 15233. Springer, Cham. https://doi.org/10.1007/978-3-031-77847-6_10</dct:bibliographicCitation>
    <dct:publisher rdf:resource="https://www.w3.org/"/>
    <foaf:logo rdf:resource="https://w3id.org/dpv/media/logo.png"/>
    <dct:contributor rdf:nodeID="person-beatriz-esteves"/>
    <dct:license rdf:resource="https://www.w3.org/copyright/document-license-2023/"/>
    <vann:preferredNamespacePrefix>eu-ehds</vann:preferredNamespacePrefix>
    <vann:preferredNamespaceUri>https://w3id.org/dpv/legal/eu/ehds#</vann:preferredNamespaceUri>
    <profile:isProfileOf rdf:resource="http://www.w3.org/2000/01/rdf-schema#"/>
    <profile:isProfileOf rdf:resource="http://www.w3.org/2004/02/skos/core#"/>
    <profile:isProfileOf rdf:resource="https://w3id.org/dpv"/>
    <profile:hasResource rdf:resource="https://w3id.org/dpv/primer"/>
    <profile:hasResource rdf:resource="https://w3id.org/dpv/guides"/>
    <profile:hasResource rdf:resource="https://w3id.org/dpv/examples"/>
    <profile:hasResource rdf:resource="https://w3id.org/dpv/legal/eu/ehds#serialisation-html"/>
    <profile:hasResource rdf:resource="https://w3id.org/dpv/legal/eu/ehds#serialisation-rdf"/>
    <profile:hasResource rdf:resource="https://w3id.org/dpv/legal/eu/ehds#serialisation-ttl"/>
    <profile:hasResource rdf:resource="https://w3id.org/dpv/legal/eu/ehds#serialisation-n3"/>
    <profile:hasResource rdf:resource="https://w3id.org/dpv/legal/eu/ehds#serialisation-jsonld"/>
  </rdf:Description>
  <rdf:Description rdf:about="https://w3id.org/dpv/legal/eu/ehds#A100">
    <rdf:type rdf:resource="http://www.w3.org/2004/02/skos/core#Concept"/>
    <rdf:type rdf:resource="http://www.w3.org/2000/01/rdf-schema#Class"/>
    <rdf:type rdf:resource="https://w3id.org/dpv#Right"/>
    <skos:prefLabel xml:lang="en">A100 Right to receive compensation</skos:prefLabel>
    <skos:definition xml:lang="en">Right of natural and legal persons to receive compensation in accordance with EU and national law in case that they have suffered material or non-material damage as a result of an infringement of the EHDS Regulation</skos:definition>
    <skos:broader rdf:resource="https://w3id.org/dpv#Right"/>
    <dct:source xml:lang="en">EHDS Art.100</dct:source>
    <dct:created rdf:datatype="http://www.w3.org/2001/XMLSchema#date">2025-10-28</dct:created>
    <sw:term_status xml:lang="en">accepted</sw:term_status>
    <dct:contributor rdf:nodeID="person-beatriz-esteves"/>
    <rdfs:isDefinedBy rdf:resource="https://w3id.org/dpv/legal/eu/ehds#"/>
    <skos:inScheme rdf:resource="https://w3id.org/dpv/legal/eu/ehds#rights-classes"/>
  </rdf:Description>
  <rdf:Description rdf:about="https://w3id.org/dpv/legal/eu/ehds#A9">
    <rdf:type rdf:resource="http://www.w3.org/2004/02/skos/core#Concept"/>
    <rdf:type rdf:resource="http://www.w3.org/2000/01/rdf-schema#Class"/>
    <rdf:type rdf:resource="https://w3id.org/dpv#Right"/>
    <skos:prefLabel xml:lang="en">A9 Right to obtain information on accessing data</skos:prefLabel>
    <skos:definition xml:lang="en">Right of natural persons to obtain information, including through automatic notifications, on any access to their personal electronic health data through the health professional access service obtained in the context of healthcare</skos:definition>
    <skos:broader rdf:resource="https://w3id.org/dpv#Right"/>
    <dct:source xml:lang="en">EHDS Art.9</dct:source>
    <dct:created rdf:datatype="http://www.w3.org/2001/XMLSchema#date">2025-10-28</dct:created>
    <sw:term_status xml:lang="en">accepted</sw:term_status>
    <dct:contributor rdf:nodeID="person-beatriz-esteves"/>
    <rdfs:isDefinedBy rdf:resource="https://w3id.org/dpv/legal/eu/ehds#"/>
    <skos:inScheme rdf:resource="https://w3id.org/dpv/legal/eu/ehds#rights-classes"/>
  </rdf:Description>
  <rdf:Description rdf:about="https://w3id.org/dpv/examples">
    <rdf:type rdf:resource="http://www.w3.org/ns/dx/prof/ResourceDescriptor"/>
    <profile:hasRole rdf:resource="http://www.w3.org/ns/dx/prof/role/guidance"/>
    <profile:hasArtifact rdf:resource="https://w3id.org/dpv/examples"/>
    <dct:title>Examples</dct:title>
    <dct:format rdf:resource="https://www.iana.org/assignments/media-types/text/html"/>
    <dct:conformsTo rdf:resource="https://www.w3.org/TR/html/"/>
  </rdf:Description>
  <rdf:Description rdf:about="https://w3id.org/dpv/legal/eu/ehds#A6">
    <rdf:type rdf:resource="http://www.w3.org/2004/02/skos/core#Concept"/>
    <rdf:type rdf:resource="http://www.w3.org/2000/01/rdf-schema#Class"/>
    <rdf:type rdf:resource="https://w3id.org/dpv#Right"/>
    <skos:prefLabel xml:lang="en">A6 Right of natural persons to rectification</skos:prefLabel>
    <skos:definition xml:lang="en">Right of natural persons to request online the rectification of their personal electronic health data</skos:definition>
    <skos:broader rdf:resource="https://w3id.org/dpv#Right"/>
    <dct:source xml:lang="en">EHDS Art.6</dct:source>
    <dct:created rdf:datatype="http://www.w3.org/2001/XMLSchema#date">2025-10-28</dct:created>
    <sw:term_status xml:lang="en">accepted</sw:term_status>
    <dct:contributor rdf:nodeID="person-beatriz-esteves"/>
    <rdfs:isDefinedBy rdf:resource="https://w3id.org/dpv/legal/eu/ehds#"/>
    <skos:inScheme rdf:resource="https://w3id.org/dpv/legal/eu/ehds#rights-classes"/>
  </rdf:Description>
  <rdf:Description rdf:about="https://w3id.org/dpv/legal/eu/ehds#A5">
    <rdf:type rdf:resource="http://www.w3.org/2004/02/skos/core#Concept"/>
    <rdf:type rdf:resource="http://www.w3.org/2000/01/rdf-schema#Class"/>
    <rdf:type rdf:resource="https://w3id.org/dpv#Right"/>
    <skos:prefLabel xml:lang="en">A5 Right of natural persons to insert information in their own EHR</skos:prefLabel>
    <skos:definition xml:lang="en">Right of natural persons to insert information in their EHR through electronic health data access services or applications linked to those services</skos:definition>
    <skos:broader rdf:resource="https://w3id.org/dpv#Right"/>
    <dct:source xml:lang="en">EHDS Art.5</dct:source>
    <dct:created rdf:datatype="http://www.w3.org/2001/XMLSchema#date">2025-10-28</dct:created>
    <sw:term_status xml:lang="en">accepted</sw:term_status>
    <dct:contributor rdf:nodeID="person-beatriz-esteves"/>
    <rdfs:isDefinedBy rdf:resource="https://w3id.org/dpv/legal/eu/ehds#"/>
    <skos:inScheme rdf:resource="https://w3id.org/dpv/legal/eu/ehds#rights-classes"/>
  </rdf:Description>
  <rdf:Description rdf:nodeID="person-beatriz-esteves">
    <rdf:type rdf:resource="http://xmlns.com/foaf/0.1/Person"/>
    <rdf:type rdf:resource="http://purl.org/dc/terms/Agent"/>
    <foaf:name>Beatriz Esteves</foaf:name>
    <scoro:hasORCID>0000-0003-0259-7560</scoro:hasORCID>
    <foaf:homepage>https://w3id.org/people/besteves</foaf:homepage>
    <org:memberOf rdf:nodeID="org-idlab-imec-ghent-university"/>
  </rdf:Description>
  <rdf:Description rdf:about="https://w3id.org/dpv/legal/eu/ehds#A3">
    <rdf:type rdf:resource="http://www.w3.org/2004/02/skos/core#Concept"/>
    <rdf:type rdf:resource="http://www.w3.org/2000/01/rdf-schema#Class"/>
    <rdf:type rdf:resource="https://w3id.org/dpv#Right"/>
    <skos:prefLabel xml:lang="en">A3 Right of natural persons to access their personal electronic health data</skos:prefLabel>
    <skos:definition xml:lang="en">Right of natural persons to access personal electronic health data relating to them that belong to the priority categories referred to in Article 14 and are processed for the provision of healthcare through the electronic health data access services referred to in Article 4</skos:definition>
    <skos:broader rdf:resource="https://w3id.org/dpv#Right"/>
    <dct:source xml:lang="en">EHDS Art.3</dct:source>
    <dct:created rdf:datatype="http://www.w3.org/2001/XMLSchema#date">2025-10-28</dct:created>
    <sw:term_status xml:lang="en">accepted</sw:term_status>
    <dct:contributor rdf:nodeID="person-beatriz-esteves"/>
    <rdfs:isDefinedBy rdf:resource="https://w3id.org/dpv/legal/eu/ehds#"/>
    <skos:inScheme rdf:resource="https://w3id.org/dpv/legal/eu/ehds#rights-classes"/>
  </rdf:Description>
  <rdf:Description rdf:about="https://w3id.org/dpv/legal/eu/ehds#A7">
    <rdf:type rdf:resource="http://www.w3.org/2004/02/skos/core#Concept"/>
    <rdf:type rdf:resource="http://www.w3.org/2000/01/rdf-schema#Class"/>
    <rdf:type rdf:resource="https://w3id.org/dpv#Right"/>
    <skos:prefLabel xml:lang="en">A7 Right to data portability for natural persons</skos:prefLabel>
    <skos:definition xml:lang="en">Right of natural persons to give access to, or to request a healthcare provider to transmit, all or part of their personal electronic health data to another healthcare provider of their choice</skos:definition>
    <skos:broader rdf:resource="https://w3id.org/dpv#Right"/>
    <dct:source xml:lang="en">EHDS Art.7</dct:source>
    <dct:created rdf:datatype="http://www.w3.org/2001/XMLSchema#date">2025-10-28</dct:created>
    <sw:term_status xml:lang="en">accepted</sw:term_status>
    <dct:contributor rdf:nodeID="person-beatriz-esteves"/>
    <rdfs:isDefinedBy rdf:resource="https://w3id.org/dpv/legal/eu/ehds#"/>
    <skos:inScheme rdf:resource="https://w3id.org/dpv/legal/eu/ehds#rights-classes"/>
  </rdf:Description>
  <rdf:Description rdf:about="https://w3id.org/dpv/legal/eu/ehds#A21">
    <rdf:type rdf:resource="http://www.w3.org/2004/02/skos/core#Concept"/>
    <rdf:type rdf:resource="http://www.w3.org/2000/01/rdf-schema#Class"/>
    <rdf:type rdf:resource="https://w3id.org/dpv#Right"/>
    <skos:prefLabel xml:lang="en">A21 Right to lodge a complaint with a digital health authority</skos:prefLabel>
    <skos:definition xml:lang="en">Right of natural and legal persons to lodge a complaint with the competent digital health authority</skos:definition>
    <skos:broader rdf:resource="https://w3id.org/dpv#Right"/>
    <dct:source xml:lang="en">EHDS Art.21</dct:source>
    <dct:created rdf:datatype="http://www.w3.org/2001/XMLSchema#date">2025-10-28</dct:created>
    <sw:term_status xml:lang="en">accepted</sw:term_status>
    <dct:contributor rdf:nodeID="person-beatriz-esteves"/>
    <rdfs:isDefinedBy rdf:resource="https://w3id.org/dpv/legal/eu/ehds#"/>
    <skos:inScheme rdf:resource="https://w3id.org/dpv/legal/eu/ehds#rights-classes"/>
  </rdf:Description>
  <rdf:Description rdf:about="https://w3id.org/dpv/legal/eu/ehds#serialisation-jsonld">
    <rdf:type rdf:resource="http://www.w3.org/ns/dx/prof/ResourceDescriptor"/>
    <profile:hasRole rdf:resource="http://www.w3.org/ns/dx/prof/role/vocabulary"/>
    <profile:hasArtifact rdf:resource="https://w3id.org/dpv/legal/eu/ehds/eu-ehds.jsonld"/>
    <dct:format rdf:resource="https://www.iana.org/assignments/media-types/application/ld+json"/>
    <dct:conformsTo rdf:resource="https://www.w3.org/TR/json-ld11/"/>
    <dct:title>EU European Health Data Spaces (EHDS) - JSON-LD serialisation</dct:title>
  </rdf:Description>
  <rdf:Description rdf:about="https://w3id.org/dpv/legal/eu/ehds#A71">
    <rdf:type rdf:resource="http://www.w3.org/2004/02/skos/core#Concept"/>
    <rdf:type rdf:resource="http://www.w3.org/2000/01/rdf-schema#Class"/>
    <rdf:type rdf:resource="https://w3id.org/dpv#Right"/>
    <skos:prefLabel xml:lang="en">A71 Right of natural persons to opt out from secondary use</skos:prefLabel>
    <skos:definition xml:lang="en">Right of natural persons to opt out at any time, and without providing any reason, from the processing of personal electronic health data relating to them for secondary use</skos:definition>
    <skos:broader rdf:resource="https://w3id.org/dpv#Right"/>
    <dct:source xml:lang="en">EHDS Art.71</dct:source>
    <dct:created rdf:datatype="http://www.w3.org/2001/XMLSchema#date">2025-10-28</dct:created>
    <sw:term_status xml:lang="en">accepted</sw:term_status>
    <dct:contributor rdf:nodeID="person-beatriz-esteves"/>
    <rdfs:isDefinedBy rdf:resource="https://w3id.org/dpv/legal/eu/ehds#"/>
    <skos:inScheme rdf:resource="https://w3id.org/dpv/legal/eu/ehds#rights-classes"/>
  </rdf:Description>
  <rdf:Description rdf:nodeID="person-harshvardhan-j-pandit">
    <rdf:type rdf:resource="http://xmlns.com/foaf/0.1/Person"/>
    <rdf:type rdf:resource="http://purl.org/dc/terms/Agent"/>
    <foaf:name>Harshvardhan J. Pandit</foaf:name>
    <scoro:hasORCID>0000-0002-5068-3714</scoro:hasORCID>
    <foaf:homepage>https://harshp.com/</foaf:homepage>
    <org:memberOf rdf:nodeID="org-ai-accountability-lab-aial-trinity-college-dublin"/>
  </rdf:Description>
  <rdf:Description rdf:nodeID="org-idlab-imec-ghent-university">
    <rdf:type rdf:resource="http://xmlns.com/foaf/0.1/Organization"/>
    <foaf:name>IDLab, IMEC, Ghent University</foaf:name>
  </rdf:Description>
  <rdf:Description rdf:about="https://w3id.org/dpv/guides">
    <rdf:type rdf:resource="http://www.w3.org/ns/dx/prof/ResourceDescriptor"/>
    <profile:hasRole rdf:resource="http://www.w3.org/ns/dx/prof/role/guidance"/>
    <profile:hasArtifact rdf:resource="https://w3id.org/dpv/guides"/>
    <dct:title>Guides for Data Privacy Vocabulary</dct:title>
    <dct:format rdf:resource="https://www.iana.org/assignments/media-types/text/html"/>
    <dct:conformsTo rdf:resource="https://www.w3.org/TR/html/"/>
  </rdf:Description>
  <rdf:Description rdf:about="https://w3id.org/dpv/legal/eu/ehds#serialisation-rdf">
    <rdf:type rdf:resource="http://www.w3.org/ns/dx/prof/ResourceDescriptor"/>
    <profile:hasRole rdf:resource="http://www.w3.org/ns/dx/prof/role/vocabulary"/>
    <profile:hasArtifact rdf:resource="https://w3id.org/dpv/legal/eu/ehds/eu-ehds.rdf"/>
    <dct:format rdf:resource="https://www.iana.org/assignments/media-types/application/rdf+xml"/>
    <dct:conformsTo rdf:resource="http://www.w3.org/1999/02/22-rdf-syntax-ns#"/>
    <dct:title>EU European Health Data Spaces (EHDS) - RDF/XML serialisation</dct:title>
  </rdf:Description>
  <rdf:Description rdf:about="https://w3id.org/dpv/legal/eu/ehds#serialisation-n3">
    <rdf:type rdf:resource="http://www.w3.org/ns/dx/prof/ResourceDescriptor"/>
    <profile:hasRole rdf:resource="http://www.w3.org/ns/dx/prof/role/vocabulary"/>
    <profile:hasArtifact rdf:resource="https://w3id.org/dpv/legal/eu/ehds/eu-ehds.n3"/>
    <dct:format rdf:resource="https://www.iana.org/assignments/media-types/text/n3"/>
    <dct:conformsTo rdf:resource="https://www.w3.org/TeamSubmission/n3/"/>
    <dct:title>EU European Health Data Spaces (EHDS) - N3 serialisation</dct:title>
  </rdf:Description>
  <rdf:Description rdf:about="https://w3id.org/dpv/primer">
    <profile:hasRole rdf:resource="http://www.w3.org/ns/dx/prof/role/guidance"/>
    <rdf:type rdf:resource="http://www.w3.org/ns/dx/prof/ResourceDescriptor"/>
    <profile:hasArtifact rdf:resource="https://w3id.org/dpv/primer"/>
    <dct:title>Primer for Data Privacy Vocabulary</dct:title>
    <dct:format rdf:resource="https://www.iana.org/assignments/media-types/text/html"/>
    <dct:conformsTo rdf:resource="https://www.w3.org/TR/html/"/>
  </rdf:Description>
  <rdf:Description rdf:about="https://w3id.org/dpv/legal/eu/ehds#rights-classes">
    <rdf:type rdf:resource="http://www.w3.org/2004/02/skos/core#ConceptScheme"/>
  </rdf:Description>
  <rdf:Description rdf:nodeID="org-ai-accountability-lab-aial-trinity-college-dublin">
    <rdf:type rdf:resource="http://xmlns.com/foaf/0.1/Organization"/>
    <foaf:name>AI Accountability Lab (AIAL), Trinity College Dublin</foaf:name>
  </rdf:Description>
</rdf:RDF>
