<?xml version="1.0" encoding="utf-8"?>
<rdf:RDF
   xmlns:bibo="http://purl.org/ontology/bibo/"
   xmlns:dct="http://purl.org/dc/terms/"
   xmlns:foaf="http://xmlns.com/foaf/0.1/"
   xmlns:org="http://www.w3.org/ns/org#"
   xmlns:owl="http://www.w3.org/2002/07/owl#"
   xmlns:profile="http://www.w3.org/ns/dx/prof/"
   xmlns:rdf="http://www.w3.org/1999/02/22-rdf-syntax-ns#"
   xmlns:rdfs="http://www.w3.org/2000/01/rdf-schema#"
   xmlns:schema="https://schema.org/"
   xmlns:scoro="http://purl.org/spar/scoro/"
   xmlns:skos="http://www.w3.org/2004/02/skos/core#"
   xmlns:sw="http://www.w3.org/2003/06/sw-vocab-status/ns#"
   xmlns:vann="http://purl.org/vocab/vann/"
>
  <rdf:Description rdf:about="https://w3id.org/dpv/legal/eu/ehds/owl#A100">
    <rdf:type rdf:resource="http://www.w3.org/2000/01/rdf-schema#Class"/>
    <rdf:type rdf:resource="https://w3id.org/dpv/owl#Right"/>
    <rdf:type rdf:resource="http://www.w3.org/2002/07/owl#Class"/>
    <dct:contributor rdf:nodeID="person-beatriz-esteves"/>
    <skos:definition xml:lang="en">Right of natural and legal persons to receive compensation in accordance with EU and national law in case that they have suffered material or non-material damage as a result of an infringement of the EHDS Regulation</skos:definition>
    <dct:created rdf:datatype="http://www.w3.org/2001/XMLSchema#date">2025-10-28</dct:created>
    <rdfs:isDefinedBy rdf:resource="https://w3id.org/dpv/legal/eu/ehds/owl#"/>
    <skos:prefLabel xml:lang="en">A100 Right to receive compensation</skos:prefLabel>
    <dct:source xml:lang="en">EHDS Art.100</dct:source>
    <sw:term_status xml:lang="en">accepted</sw:term_status>
    <rdfs:subClassOf rdf:resource="https://w3id.org/dpv/owl#Right"/>
  </rdf:Description>
  <rdf:Description rdf:about="https://w3id.org/dpv/legal/eu/ehds/owl#">
    <owl:versionIRI rdf:resource="https://w3id.org/dpv/2.3/legal/eu/ehds/owl#"/>
    <profile:isProfileOf rdf:resource="https://w3id.org/dpv/owl"/>
    <profile:isProfileOf rdf:resource="http://www.w3.org/2002/07/owl"/>
    <profile:isProfileOf rdf:resource="https://w3id.org/dpv/legal/eu/ehds/owl#"/>
    <profile:hasResource rdf:resource="https://w3id.org/dpv/guides"/>
    <profile:hasResource rdf:resource="https://w3id.org/dpv/legal/eu/ehds/owl#serialisation-jsonld"/>
    <profile:hasResource rdf:resource="https://w3id.org/dpv/legal/eu/ehds/owl#serialisation-ttl"/>
    <profile:hasResource rdf:resource="https://w3id.org/dpv/examples"/>
    <profile:hasResource rdf:resource="https://w3id.org/dpv/legal/eu/ehds/owl#serialisation-n3"/>
    <profile:hasResource rdf:resource="https://w3id.org/dpv/legal/eu/ehds/owl#serialisation-html"/>
    <profile:hasResource rdf:resource="https://w3id.org/dpv/legal/eu/ehds/owl#serialisation-rdf"/>
    <profile:hasResource rdf:resource="https://w3id.org/dpv/primer"/>
    <dct:identifier>https://w3id.org/dpv/legal/eu/ehds</dct:identifier>
    <dct:conformsTo>http://www.w3.org/2004/02/skos/core</dct:conformsTo>
    <dct:conformsTo rdf:resource="http://www.w3.org/2002/07/owl"/>
    <dct:conformsTo>http://www.w3.org/2000/01/rdf-schema</dct:conformsTo>
    <dct:title xml:lang="en">EU European Health Data Spaces (EHDS)</dct:title>
    <dct:issued xml:lang="en">2024-12-01</dct:issued>
    <dct:hasVersion rdf:resource="https://w3id.org/dpv/legal/eu/ehds/owl#"/>
    <vann:preferredNamespaceUri>https://w3id.org/dpv/legal/eu/ehds#</vann:preferredNamespaceUri>
    <dct:creator rdf:nodeID="person-harshvardhan-j-pandit"/>
    <dct:creator rdf:nodeID="person-beatriz-esteves"/>
    <dct:source rdf:resource="https://www.w3.org/groups/cg/dpvcg/"/>
    <dct:created xml:lang="en">2024-12-01</dct:created>
    <rdf:type rdf:resource="http://www.w3.org/2002/07/owl#Ontology"/>
    <rdf:type rdf:resource="http://www.w3.org/ns/dx/prof/Profile"/>
    <rdfs:Label xml:lang="en">EU-EHDS</rdfs:Label>
    <schema:version>2.3</schema:version>
    <foaf:logo rdf:resource="https://w3id.org/dpv/media/logo.png"/>
    <bibo:status>http://purl.org/ontology/bibo/status/draft</bibo:status>
    <dct:publisher rdf:resource="https://www.w3.org/"/>
    <dct:license rdf:resource="https://www.w3.org/copyright/document-license-2023/"/>
    <dct:modified xml:lang="en">2026-02-25</dct:modified>
    <dct:contributor rdf:nodeID="person-beatriz-esteves"/>
    <vann:preferredNamespacePrefix>eu-ehds</vann:preferredNamespacePrefix>
    <dct:description xml:lang="en">Extension to the Data Privacy Vocabulary (DPV) providing concepts for representing information associated with EU Health Data Spaces (EHDS)</dct:description>
    <bibo:doi>10.5281/zenodo.12505841</bibo:doi>
    <dct:bibliographicCitation>Harshvardhan J. Pandit, Beatriz Esteves, Georg P. Krog, Paul Ryan, Delaram Golpayegani, Julian Flake (2025) Data Privacy Vocabulary (DPV) – Version 2.0. In: Demartini, G., et al. The Semantic Web – ISWC 2024. ISWC 2024. Lecture Notes in Computer Science, vol 15233. Springer, Cham. https://doi.org/10.1007/978-3-031-77847-6_10</dct:bibliographicCitation>
    <owl:versionInfo>2.3</owl:versionInfo>
  </rdf:Description>
  <rdf:Description rdf:about="https://w3id.org/dpv/legal/eu/ehds/owl#A9">
    <rdf:type rdf:resource="http://www.w3.org/2000/01/rdf-schema#Class"/>
    <rdf:type rdf:resource="https://w3id.org/dpv/owl#Right"/>
    <rdf:type rdf:resource="http://www.w3.org/2002/07/owl#Class"/>
    <skos:definition xml:lang="en">Right of natural persons to obtain information, including through automatic notifications, on any access to their personal electronic health data through the health professional access service obtained in the context of healthcare</skos:definition>
    <skos:prefLabel xml:lang="en">A9 Right to obtain information on accessing data</skos:prefLabel>
    <dct:contributor rdf:nodeID="person-beatriz-esteves"/>
    <dct:created rdf:datatype="http://www.w3.org/2001/XMLSchema#date">2025-10-28</dct:created>
    <dct:source xml:lang="en">EHDS Art.9</dct:source>
    <rdfs:isDefinedBy rdf:resource="https://w3id.org/dpv/legal/eu/ehds/owl#"/>
    <sw:term_status xml:lang="en">accepted</sw:term_status>
    <rdfs:subClassOf rdf:resource="https://w3id.org/dpv/owl#Right"/>
  </rdf:Description>
  <rdf:Description rdf:about="https://w3id.org/dpv/legal/eu/ehds/owl#A6">
    <rdfs:isDefinedBy rdf:resource="https://w3id.org/dpv/legal/eu/ehds/owl#"/>
    <rdf:type rdf:resource="http://www.w3.org/2000/01/rdf-schema#Class"/>
    <rdf:type rdf:resource="https://w3id.org/dpv/owl#Right"/>
    <rdf:type rdf:resource="http://www.w3.org/2002/07/owl#Class"/>
    <dct:source xml:lang="en">EHDS Art.6</dct:source>
    <dct:contributor rdf:nodeID="person-beatriz-esteves"/>
    <dct:created rdf:datatype="http://www.w3.org/2001/XMLSchema#date">2025-10-28</dct:created>
    <skos:definition xml:lang="en">Right of natural persons to request online the rectification of their personal electronic health data</skos:definition>
    <skos:prefLabel xml:lang="en">A6 Right of natural persons to rectification</skos:prefLabel>
    <sw:term_status xml:lang="en">accepted</sw:term_status>
    <rdfs:subClassOf rdf:resource="https://w3id.org/dpv/owl#Right"/>
  </rdf:Description>
  <rdf:Description rdf:about="https://w3id.org/dpv/examples">
    <profile:hasArtifact rdf:resource="https://w3id.org/dpv/examples"/>
    <profile:hasRole rdf:resource="http://www.w3.org/ns/dx/prof/role/guidance"/>
    <dct:title>Examples</dct:title>
    <dct:format rdf:resource="https://www.iana.org/assignments/media-types/text/html"/>
    <dct:conformsTo rdf:resource="https://www.w3.org/TR/html/"/>
    <rdf:type rdf:resource="http://www.w3.org/ns/dx/prof/ResourceDescriptor"/>
  </rdf:Description>
  <rdf:Description rdf:about="https://w3id.org/dpv/legal/eu/ehds/owl#A8">
    <dct:contributor rdf:nodeID="person-beatriz-esteves"/>
    <sw:term_status xml:lang="en">accepted</sw:term_status>
    <skos:prefLabel xml:lang="en">A8 Right to restrict access</skos:prefLabel>
    <rdf:type rdf:resource="http://www.w3.org/2000/01/rdf-schema#Class"/>
    <rdf:type rdf:resource="https://w3id.org/dpv/owl#Right"/>
    <rdf:type rdf:resource="http://www.w3.org/2002/07/owl#Class"/>
    <dct:source xml:lang="en">EHDS Art.8</dct:source>
    <dct:created rdf:datatype="http://www.w3.org/2001/XMLSchema#date">2025-10-28</dct:created>
    <skos:definition xml:lang="en">Right of natural persons to restrict the access of health professionals and healthcare providers to all or parts of their personal electronic health data</skos:definition>
    <rdfs:isDefinedBy rdf:resource="https://w3id.org/dpv/legal/eu/ehds/owl#"/>
    <rdfs:subClassOf rdf:resource="https://w3id.org/dpv/owl#Right"/>
  </rdf:Description>
  <rdf:Description rdf:about="https://w3id.org/dpv/legal/eu/ehds/owl#serialisation-n3">
    <profile:hasRole rdf:resource="http://www.w3.org/ns/dx/prof/role/vocabulary"/>
    <profile:hasArtifact rdf:resource="https://w3id.org/dpv/legal/eu/ehds/eu-ehds-owl.n3"/>
    <dct:title>EU European Health Data Spaces (EHDS) - N3 serialisation</dct:title>
    <dct:conformsTo rdf:resource="https://www.w3.org/TeamSubmission/n3/"/>
    <rdf:type rdf:resource="http://www.w3.org/ns/dx/prof/ResourceDescriptor"/>
    <dct:format rdf:resource="https://www.iana.org/assignments/media-types/text/n3"/>
  </rdf:Description>
  <rdf:Description rdf:about="https://w3id.org/dpv/legal/eu/ehds/owl#A7">
    <skos:definition xml:lang="en">Right of natural persons to give access to, or to request a healthcare provider to transmit, all or part of their personal electronic health data to another healthcare provider of their choice</skos:definition>
    <rdf:type rdf:resource="http://www.w3.org/2000/01/rdf-schema#Class"/>
    <rdf:type rdf:resource="https://w3id.org/dpv/owl#Right"/>
    <rdf:type rdf:resource="http://www.w3.org/2002/07/owl#Class"/>
    <sw:term_status xml:lang="en">accepted</sw:term_status>
    <dct:created rdf:datatype="http://www.w3.org/2001/XMLSchema#date">2025-10-28</dct:created>
    <dct:source xml:lang="en">EHDS Art.7</dct:source>
    <dct:contributor rdf:nodeID="person-beatriz-esteves"/>
    <rdfs:isDefinedBy rdf:resource="https://w3id.org/dpv/legal/eu/ehds/owl#"/>
    <skos:prefLabel xml:lang="en">A7 Right to data portability for natural persons</skos:prefLabel>
    <rdfs:subClassOf rdf:resource="https://w3id.org/dpv/owl#Right"/>
  </rdf:Description>
  <rdf:Description rdf:about="https://w3id.org/dpv/legal/eu/ehds/owl#A71">
    <sw:term_status xml:lang="en">accepted</sw:term_status>
    <rdf:type rdf:resource="http://www.w3.org/2000/01/rdf-schema#Class"/>
    <rdf:type rdf:resource="https://w3id.org/dpv/owl#Right"/>
    <rdf:type rdf:resource="http://www.w3.org/2002/07/owl#Class"/>
    <skos:prefLabel xml:lang="en">A71 Right of natural persons to opt out from secondary use</skos:prefLabel>
    <dct:contributor rdf:nodeID="person-beatriz-esteves"/>
    <rdfs:isDefinedBy rdf:resource="https://w3id.org/dpv/legal/eu/ehds/owl#"/>
    <dct:created rdf:datatype="http://www.w3.org/2001/XMLSchema#date">2025-10-28</dct:created>
    <skos:definition xml:lang="en">Right of natural persons to opt out at any time, and without providing any reason, from the processing of personal electronic health data relating to them for secondary use</skos:definition>
    <dct:source xml:lang="en">EHDS Art.71</dct:source>
    <rdfs:subClassOf rdf:resource="https://w3id.org/dpv/owl#Right"/>
  </rdf:Description>
  <rdf:Description rdf:about="https://w3id.org/dpv/legal/eu/ehds/owl#A3">
    <dct:source xml:lang="en">EHDS Art.3</dct:source>
    <rdf:type rdf:resource="http://www.w3.org/2000/01/rdf-schema#Class"/>
    <rdf:type rdf:resource="https://w3id.org/dpv/owl#Right"/>
    <rdf:type rdf:resource="http://www.w3.org/2002/07/owl#Class"/>
    <dct:contributor rdf:nodeID="person-beatriz-esteves"/>
    <dct:created rdf:datatype="http://www.w3.org/2001/XMLSchema#date">2025-10-28</dct:created>
    <rdfs:isDefinedBy rdf:resource="https://w3id.org/dpv/legal/eu/ehds/owl#"/>
    <skos:definition xml:lang="en">Right of natural persons to access personal electronic health data relating to them that belong to the priority categories referred to in Article 14 and are processed for the provision of healthcare through the electronic health data access services referred to in Article 4</skos:definition>
    <skos:prefLabel xml:lang="en">A3 Right of natural persons to access their personal electronic health data</skos:prefLabel>
    <sw:term_status xml:lang="en">accepted</sw:term_status>
    <rdfs:subClassOf rdf:resource="https://w3id.org/dpv/owl#Right"/>
  </rdf:Description>
  <rdf:Description rdf:nodeID="person-beatriz-esteves">
    <scoro:hasORCID>0000-0003-0259-7560</scoro:hasORCID>
    <rdf:type rdf:resource="http://purl.org/dc/terms/Agent"/>
    <rdf:type rdf:resource="http://xmlns.com/foaf/0.1/Person"/>
    <org:memberOf rdf:nodeID="org-idlab-imec-ghent-university"/>
    <foaf:name>Beatriz Esteves</foaf:name>
    <foaf:homepage>https://w3id.org/people/besteves</foaf:homepage>
  </rdf:Description>
  <rdf:Description rdf:about="https://w3id.org/dpv/legal/eu/ehds/owl#A16-1">
    <sw:term_status xml:lang="en">accepted</sw:term_status>
    <rdfs:isDefinedBy rdf:resource="https://w3id.org/dpv/legal/eu/ehds/owl#"/>
    <rdf:type rdf:resource="http://www.w3.org/2000/01/rdf-schema#Class"/>
    <rdf:type rdf:resource="https://w3id.org/dpv/owl#Right"/>
    <rdf:type rdf:resource="http://www.w3.org/2002/07/owl#Class"/>
    <skos:definition xml:lang="en">Right of natural persons to identify themselves electronically using any electronic identification means which are recognised pursuant to Article 6 of Regulation (EU) No 910/2014</skos:definition>
    <dct:contributor rdf:nodeID="person-beatriz-esteves"/>
    <dct:created rdf:datatype="http://www.w3.org/2001/XMLSchema#date">2025-10-28</dct:created>
    <skos:prefLabel xml:lang="en">A16-1 Right of identification management</skos:prefLabel>
    <dct:source xml:lang="en">EHDS Art.16.1</dct:source>
    <rdfs:subClassOf rdf:resource="https://w3id.org/dpv/owl#Right"/>
  </rdf:Description>
  <rdf:Description rdf:about="https://w3id.org/dpv/legal/eu/ehds/owl#A10">
    <rdf:type rdf:resource="http://www.w3.org/2000/01/rdf-schema#Class"/>
    <rdf:type rdf:resource="https://w3id.org/dpv/owl#Right"/>
    <rdf:type rdf:resource="http://www.w3.org/2002/07/owl#Class"/>
    <sw:term_status xml:lang="en">accepted</sw:term_status>
    <skos:definition xml:lang="en">Right of natural persons to opt out from the access to their personal electronic health data registered in an EHR system through the electronic health data access services</skos:definition>
    <skos:prefLabel xml:lang="en">A10 Right of natural persons to opt out from primary use</skos:prefLabel>
    <dct:contributor rdf:nodeID="person-beatriz-esteves"/>
    <dct:created rdf:datatype="http://www.w3.org/2001/XMLSchema#date">2025-10-28</dct:created>
    <dct:source xml:lang="en">EHDS Art.10</dct:source>
    <rdfs:isDefinedBy rdf:resource="https://w3id.org/dpv/legal/eu/ehds/owl#"/>
    <rdfs:subClassOf rdf:resource="https://w3id.org/dpv/owl#Right"/>
  </rdf:Description>
  <rdf:Description rdf:about="https://w3id.org/dpv/legal/eu/ehds/owl#A68-11">
    <rdfs:isDefinedBy rdf:resource="https://w3id.org/dpv/legal/eu/ehds/owl#"/>
    <rdf:type rdf:resource="http://www.w3.org/2000/01/rdf-schema#Class"/>
    <rdf:type rdf:resource="https://w3id.org/dpv/owl#Right"/>
    <rdf:type rdf:resource="http://www.w3.org/2002/07/owl#Class"/>
    <dct:contributor rdf:nodeID="person-beatriz-esteves"/>
    <skos:prefLabel xml:lang="en">A68-11 Right to process in a secure processing environment</skos:prefLabel>
    <dct:source xml:lang="en">EHDS Art.68.11</dct:source>
    <dct:created rdf:datatype="http://www.w3.org/2001/XMLSchema#date">2025-10-28</dct:created>
    <skos:definition xml:lang="en">Right of health data users to access and process the electronic health data in a secure processing environment in accordance with the data permit issued to them</skos:definition>
    <sw:term_status xml:lang="en">accepted</sw:term_status>
    <rdfs:subClassOf rdf:resource="https://w3id.org/dpv/owl#Right"/>
  </rdf:Description>
  <rdf:Description rdf:nodeID="person-harshvardhan-j-pandit">
    <scoro:hasORCID>0000-0002-5068-3714</scoro:hasORCID>
    <rdf:type rdf:resource="http://purl.org/dc/terms/Agent"/>
    <rdf:type rdf:resource="http://xmlns.com/foaf/0.1/Person"/>
    <org:memberOf rdf:nodeID="org-ai-accountability-lab-aial-trinity-college-dublin"/>
    <foaf:homepage>https://harshp.com/</foaf:homepage>
    <foaf:name>Harshvardhan J. Pandit</foaf:name>
  </rdf:Description>
  <rdf:Description rdf:about="https://w3id.org/dpv/legal/eu/ehds/owl#serialisation-ttl">
    <profile:hasRole rdf:resource="http://www.w3.org/ns/dx/prof/role/vocabulary"/>
    <dct:conformsTo rdf:resource="https://www.w3.org/TR/turtle/"/>
    <dct:format rdf:resource="https://www.iana.org/assignments/media-types/text/turtle"/>
    <dct:title>EU European Health Data Spaces (EHDS) - Turtle serialisation</dct:title>
    <profile:hasArtifact rdf:resource="https://w3id.org/dpv/legal/eu/ehds/eu-ehds-owl.ttl"/>
    <rdf:type rdf:resource="http://www.w3.org/ns/dx/prof/ResourceDescriptor"/>
  </rdf:Description>
  <rdf:Description rdf:about="https://w3id.org/dpv/legal/eu/ehds/owl#A5">
    <rdf:type rdf:resource="https://w3id.org/dpv/owl#Right"/>
    <rdf:type rdf:resource="http://www.w3.org/2000/01/rdf-schema#Class"/>
    <rdf:type rdf:resource="http://www.w3.org/2002/07/owl#Class"/>
    <skos:definition xml:lang="en">Right of natural persons to insert information in their EHR through electronic health data access services or applications linked to those services</skos:definition>
    <dct:created rdf:datatype="http://www.w3.org/2001/XMLSchema#date">2025-10-28</dct:created>
    <dct:contributor rdf:nodeID="person-beatriz-esteves"/>
    <rdfs:isDefinedBy rdf:resource="https://w3id.org/dpv/legal/eu/ehds/owl#"/>
    <dct:source xml:lang="en">EHDS Art.5</dct:source>
    <sw:term_status xml:lang="en">accepted</sw:term_status>
    <skos:prefLabel xml:lang="en">A5 Right of natural persons to insert information in their own EHR</skos:prefLabel>
    <rdfs:subClassOf rdf:resource="https://w3id.org/dpv/owl#Right"/>
  </rdf:Description>
  <rdf:Description rdf:nodeID="org-idlab-imec-ghent-university">
    <rdf:type rdf:resource="http://xmlns.com/foaf/0.1/Organization"/>
    <foaf:name>IDLab, IMEC, Ghent University</foaf:name>
  </rdf:Description>
  <rdf:Description rdf:about="https://w3id.org/dpv/legal/eu/ehds/owl#A21">
    <dct:created rdf:datatype="http://www.w3.org/2001/XMLSchema#date">2025-10-28</dct:created>
    <skos:definition xml:lang="en">Right of natural and legal persons to lodge a complaint with the competent digital health authority</skos:definition>
    <rdf:type rdf:resource="http://www.w3.org/2000/01/rdf-schema#Class"/>
    <rdf:type rdf:resource="https://w3id.org/dpv/owl#Right"/>
    <rdf:type rdf:resource="http://www.w3.org/2002/07/owl#Class"/>
    <sw:term_status xml:lang="en">accepted</sw:term_status>
    <dct:source xml:lang="en">EHDS Art.21</dct:source>
    <rdfs:isDefinedBy rdf:resource="https://w3id.org/dpv/legal/eu/ehds/owl#"/>
    <skos:prefLabel xml:lang="en">A21 Right to lodge a complaint with a digital health authority</skos:prefLabel>
    <dct:contributor rdf:nodeID="person-beatriz-esteves"/>
    <rdfs:subClassOf rdf:resource="https://w3id.org/dpv/owl#Right"/>
  </rdf:Description>
  <rdf:Description rdf:about="https://w3id.org/dpv/legal/eu/ehds/owl#serialisation-rdf">
    <profile:hasRole rdf:resource="http://www.w3.org/ns/dx/prof/role/vocabulary"/>
    <profile:hasArtifact rdf:resource="https://w3id.org/dpv/legal/eu/ehds/eu-ehds-owl.rdf"/>
    <dct:conformsTo rdf:resource="http://www.w3.org/1999/02/22-rdf-syntax-ns#"/>
    <dct:format rdf:resource="https://www.iana.org/assignments/media-types/application/rdf+xml"/>
    <rdf:type rdf:resource="http://www.w3.org/ns/dx/prof/ResourceDescriptor"/>
    <dct:title>EU European Health Data Spaces (EHDS) - RDF/XML serialisation</dct:title>
  </rdf:Description>
  <rdf:Description rdf:about="https://w3id.org/dpv/guides">
    <profile:hasArtifact rdf:resource="https://w3id.org/dpv/guides"/>
    <dct:format rdf:resource="https://www.iana.org/assignments/media-types/text/html"/>
    <profile:hasRole rdf:resource="http://www.w3.org/ns/dx/prof/role/guidance"/>
    <dct:conformsTo rdf:resource="https://www.w3.org/TR/html/"/>
    <rdf:type rdf:resource="http://www.w3.org/ns/dx/prof/ResourceDescriptor"/>
    <dct:title>Guides for Data Privacy Vocabulary</dct:title>
  </rdf:Description>
  <rdf:Description rdf:about="https://w3id.org/dpv/legal/eu/ehds/owl#serialisation-jsonld">
    <dct:title>EU European Health Data Spaces (EHDS) - JSON-LD serialisation</dct:title>
    <dct:conformsTo rdf:resource="https://www.w3.org/TR/json-ld11/"/>
    <profile:hasArtifact rdf:resource="https://w3id.org/dpv/legal/eu/ehds/eu-ehds-owl.jsonld"/>
    <dct:format rdf:resource="https://www.iana.org/assignments/media-types/application/ld+json"/>
    <profile:hasRole rdf:resource="http://www.w3.org/ns/dx/prof/role/vocabulary"/>
    <rdf:type rdf:resource="http://www.w3.org/ns/dx/prof/ResourceDescriptor"/>
  </rdf:Description>
  <rdf:Description rdf:about="https://w3id.org/dpv/primer">
    <rdf:type rdf:resource="http://www.w3.org/ns/dx/prof/ResourceDescriptor"/>
    <profile:hasRole rdf:resource="http://www.w3.org/ns/dx/prof/role/guidance"/>
    <dct:format rdf:resource="https://www.iana.org/assignments/media-types/text/html"/>
    <dct:conformsTo rdf:resource="https://www.w3.org/TR/html/"/>
    <profile:hasArtifact rdf:resource="https://w3id.org/dpv/primer"/>
    <dct:title>Primer for Data Privacy Vocabulary</dct:title>
  </rdf:Description>
  <rdf:Description rdf:about="https://w3id.org/dpv/legal/eu/ehds/owl#serialisation-html">
    <dct:conformsTo rdf:resource="https://www.w3.org/TR/html/"/>
    <dct:title>EU European Health Data Spaces (EHDS) - HTML serialisation</dct:title>
    <rdf:type rdf:resource="http://www.w3.org/ns/dx/prof/ResourceDescriptor"/>
    <profile:hasRole rdf:resource="http://www.w3.org/ns/dx/prof/role/specification"/>
    <profile:hasArtifact rdf:resource="https://w3id.org/dpv/legal/eu/ehds/eu-ehds-owl.html"/>
    <dct:format rdf:resource="https://www.iana.org/assignments/media-types/text/html"/>
  </rdf:Description>
  <rdf:Description rdf:nodeID="org-ai-accountability-lab-aial-trinity-college-dublin">
    <foaf:name>AI Accountability Lab (AIAL), Trinity College Dublin</foaf:name>
    <rdf:type rdf:resource="http://xmlns.com/foaf/0.1/Organization"/>
  </rdf:Description>
</rdf:RDF>
