@prefix bibo: <http://purl.org/ontology/bibo/> .
@prefix dct: <http://purl.org/dc/terms/> .
@prefix dpv: <https://w3id.org/dpv#> .
@prefix eu-ehds: <https://w3id.org/dpv/legal/eu/ehds#> .
@prefix foaf: <http://xmlns.com/foaf/0.1/> .
@prefix org: <http://www.w3.org/ns/org#> .
@prefix owl: <http://www.w3.org/2002/07/owl#> .
@prefix profile: <http://www.w3.org/ns/dx/prof/> .
@prefix rdfs: <http://www.w3.org/2000/01/rdf-schema#> .
@prefix role: <http://www.w3.org/ns/dx/prof/role/> .
@prefix schema: <https://schema.org/> .
@prefix scoro: <http://purl.org/spar/scoro/> .
@prefix skos: <http://www.w3.org/2004/02/skos/core#> .
@prefix sw: <http://www.w3.org/2003/06/sw-vocab-status/ns#> .
@prefix vann: <http://purl.org/vocab/vann/> .
@prefix xsd: <http://www.w3.org/2001/XMLSchema#> .

eu-ehds:DigitalHealthAuthorityActivityReport a rdfs:Class,
        skos:Concept,
        dpv:OrganisationalMeasure ;
    dct:contributor _:person-beatriz-esteves ;
    dct:created "2025-10-28"^^xsd:date ;
    dct:source "EHDS Art.20"@en ;
    rdfs:isDefinedBy eu-ehds: ;
    sw:term_status "accepted"@en ;
    skos:broader dpv:RecordsOfActivities ;
    skos:definition "Document containing an overview of activities reported by a digital health authority"@en ;
    skos:inScheme eu-ehds:TOM-classes ;
    skos:prefLabel "Digital Health Authority Activity Report"@en .

eu-ehds:EHRSystemInformationSheet a rdfs:Class,
        skos:Concept,
        dpv:OrganisationalMeasure ;
    dct:contributor _:person-beatriz-esteves ;
    dct:created "2025-10-28"^^xsd:date ;
    dct:source "EHDS Art.38"@en ;
    rdfs:isDefinedBy eu-ehds: ;
    sw:term_status "accepted"@en ;
    skos:broader dpv:OrganisationalMeasure ;
    skos:definition "Technical documentation with information related to the EHR system, including its manufacturer, intended purpose and supported standards"@en ;
    skos:inScheme eu-ehds:TOM-classes ;
    skos:prefLabel "EHR System Information Sheet"@en .

eu-ehds:EHRSystemTechnicalDocumentation a rdfs:Class,
        skos:Concept,
        dpv:OrganisationalMeasure ;
    dct:contributor _:person-beatriz-esteves ;
    dct:created "2025-10-28"^^xsd:date ;
    dct:source "EHDS Art.37"@en ;
    rdfs:isDefinedBy eu-ehds: ;
    sw:term_status "accepted"@en ;
    skos:broader dpv:OrganisationalMeasure ;
    skos:definition "Technical documentation that demonstrates that the EHR system manufacturers comply with the requirements laid down in Annex II"@en ;
    skos:inScheme eu-ehds:TOM-classes ;
    skos:prefLabel "EHR System Technical Documentation"@en .

eu-ehds:EUDatabaseForRegistrationOfEHRSystems a rdfs:Class,
        skos:Concept,
        dpv:OrganisationalMeasure ;
    dct:contributor _:person-beatriz-esteves ;
    dct:created "2025-10-28"^^xsd:date ;
    dct:source "EHDS Art.49"@en ;
    rdfs:isDefinedBy eu-ehds: ;
    sw:term_status "accepted"@en ;
    skos:broader dpv:OrganisationalMeasure ;
    skos:definition "Publicly available database established by the European Commission to maintain data on EHR systems for which an EU declaration of conformity has been issued according to EHDS Article 39"@en ;
    skos:inScheme eu-ehds:TOM-classes ;
    skos:prefLabel "EU Database for Registration of EHR Systems"@en .

eu-ehds:EUDatabaseForRegistrationOfWellnessApplications a rdfs:Class,
        skos:Concept,
        dpv:OrganisationalMeasure ;
    dct:contributor _:person-beatriz-esteves ;
    dct:created "2025-10-28"^^xsd:date ;
    dct:source "EHDS Art.49"@en ;
    rdfs:isDefinedBy eu-ehds: ;
    sw:term_status "accepted"@en ;
    skos:broader dpv:OrganisationalMeasure ;
    skos:definition "Publicly available database established by the European Commission to maintain data on wellness applications for which a label has been issued pursuant to EHDS Article 47"@en ;
    skos:inScheme eu-ehds:TOM-classes ;
    skos:prefLabel "EU Database for Registration of Wellness Applications"@en .

eu-ehds:EUDeclarationOfConformity a rdfs:Class,
        skos:Concept,
        dpv:OrganisationalMeasure ;
    dct:contributor _:person-beatriz-esteves ;
    dct:created "2025-10-28"^^xsd:date ;
    dct:source "EHDS Art.39"@en ;
    rdfs:isDefinedBy eu-ehds: ;
    sw:term_status "accepted"@en ;
    skos:broader dpv:CertificationSeal ;
    skos:definition "Declaration of conformity by the EU stating that the manufacturer of an EHR system has demonstrated that the essential requirements laid down in EHDS Annex II have been fulfilled"@en ;
    skos:inScheme eu-ehds:TOM-classes ;
    skos:prefLabel "EU Declaration of Conformity"@en .

eu-ehds:EuropeanDigitalTestingEnvironment a rdfs:Class,
        skos:Concept,
        dpv:OrganisationalMeasure ;
    dct:contributor _:person-beatriz-esteves ;
    dct:created "2025-10-28"^^xsd:date ;
    dct:source "EHDS Art.40"@en ;
    rdfs:isDefinedBy eu-ehds: ;
    sw:term_status "accepted"@en ;
    skos:broader dpv:SecureProcessingEnvironment ;
    skos:definition "Data processing environment for the assessment of harmonised software components of EHR systems"@en ;
    skos:inScheme eu-ehds:TOM-classes ;
    skos:prefLabel "European Digital Testing Environment"@en .

eu-ehds:WellnessApplicationLabel a rdfs:Class,
        skos:Concept,
        dpv:OrganisationalMeasure ;
    dct:contributor _:person-beatriz-esteves ;
    dct:created "2025-10-28"^^xsd:date ;
    dct:source "EHDS Art.47"@en ;
    rdfs:isDefinedBy eu-ehds: ;
    sw:term_status "accepted"@en ;
    skos:broader dpv:CertificationSeal ;
    skos:definition "Label issued by the manufacturer of the wellness application that indicating its compliance with the common specifications referred to in EHDS Article 36 and the requirements laid down in EHDS Annex II"@en ;
    skos:inScheme eu-ehds:TOM-classes ;
    skos:prefLabel "Wellness Application Label"@en .

<https://w3id.org/dpv/legal/eu/ehds> a owl:Ontology,
        profile:Profile ;
    dct:bibliographicCitation "Harshvardhan J. Pandit, Beatriz Esteves, Georg P. Krog, Paul Ryan, Delaram Golpayegani, Julian Flake (2025) Data Privacy Vocabulary (DPV) – Version 2.0. In: Demartini, G., et al. The Semantic Web – ISWC 2024. ISWC 2024. Lecture Notes in Computer Science, vol 15233. Springer, Cham. https://doi.org/10.1007/978-3-031-77847-6_10" ;
    dct:conformsTo "http://www.w3.org/2000/01/rdf-schema",
        "http://www.w3.org/2004/02/skos/core" ;
    dct:contributor _:person-beatriz-esteves ;
    dct:created "2024-12-01"@en ;
    dct:creator _:person-beatriz-esteves,
        [ a dct:Agent,
                foaf:Person ;
            scoro:hasORCID "0000-0002-5068-3714" ;
            org:memberOf [ a foaf:Organization ;
                    foaf:name "AI Accountability Lab (AIAL), Trinity College Dublin" ] ;
            foaf:homepage "https://harshp.com/" ;
            foaf:name "Harshvardhan J. Pandit" ] ;
    dct:description "Extension to the Data Privacy Vocabulary (DPV) providing concepts for representing information associated with EU Health Data Spaces (EHDS)"@en ;
    dct:identifier "https://w3id.org/dpv/legal/eu/ehds" ;
    dct:issued "2024-12-01"@en ;
    dct:license <https://www.w3.org/copyright/document-license-2023/> ;
    dct:modified "2026-02-25"@en ;
    dct:publisher <https://www.w3.org/> ;
    dct:source <https://www.w3.org/groups/cg/dpvcg/> ;
    dct:title "EU European Health Data Spaces (EHDS)"@en ;
    bibo:doi "10.5281/zenodo.12505841" ;
    bibo:status "http://purl.org/ontology/bibo/status/draft" ;
    vann:preferredNamespacePrefix "eu-ehds" ;
    vann:preferredNamespaceUri "https://w3id.org/dpv/legal/eu/ehds#" ;
    rdfs:Label "EU-EHDS"@en ;
    owl:versionIRI <https://w3id.org/dpv/2.3/legal/eu/ehds> ;
    owl:versionInfo "2.3" ;
    profile:hasResource <https://w3id.org/dpv/examples>,
        <https://w3id.org/dpv/guides>,
        eu-ehds:serialisation-html,
        eu-ehds:serialisation-ttl,
        <https://w3id.org/dpv/primer> ;
    profile:isProfileOf rdfs:,
        skos:,
        <https://w3id.org/dpv> ;
    foaf:logo <https://w3id.org/dpv/media/logo.png> ;
    schema:version "2.3" .

eu-ehds:serialisation-html a profile:ResourceDescriptor ;
    dct:conformsTo <https://www.w3.org/TR/html/> ;
    dct:format <https://www.iana.org/assignments/media-types/text/html> ;
    dct:title "EU European Health Data Spaces (EHDS) - HTML serialisation" ;
    profile:hasArtifact <https://w3id.org/dpv/legal/eu/ehds/eu-ehds.html> ;
    profile:hasRole role:specification .

eu-ehds:serialisation-ttl a profile:ResourceDescriptor ;
    dct:conformsTo <https://www.w3.org/TR/turtle/> ;
    dct:format <https://www.iana.org/assignments/media-types/text/turtle> ;
    dct:title "EU European Health Data Spaces (EHDS) - Turtle serialisation" ;
    profile:hasArtifact <https://w3id.org/dpv/legal/eu/ehds/eu-ehds.ttl> ;
    profile:hasRole role:vocabulary .

<https://w3id.org/dpv/examples> a profile:ResourceDescriptor ;
    dct:conformsTo <https://www.w3.org/TR/html/> ;
    dct:format <https://www.iana.org/assignments/media-types/text/html> ;
    dct:title "Examples" ;
    profile:hasArtifact <https://w3id.org/dpv/examples> ;
    profile:hasRole role:guidance .

<https://w3id.org/dpv/guides> a profile:ResourceDescriptor ;
    dct:conformsTo <https://www.w3.org/TR/html/> ;
    dct:format <https://www.iana.org/assignments/media-types/text/html> ;
    dct:title "Guides for Data Privacy Vocabulary" ;
    profile:hasArtifact <https://w3id.org/dpv/guides> ;
    profile:hasRole role:guidance .

<https://w3id.org/dpv/primer> a profile:ResourceDescriptor ;
    dct:conformsTo <https://www.w3.org/TR/html/> ;
    dct:format <https://www.iana.org/assignments/media-types/text/html> ;
    dct:title "Primer for Data Privacy Vocabulary" ;
    profile:hasArtifact <https://w3id.org/dpv/primer> ;
    profile:hasRole role:guidance .

eu-ehds:TOM-classes a skos:ConceptScheme .

_:org-idlab-imec-ghent-university a foaf:Organization ;
    foaf:name "IDLab, IMEC, Ghent University" .

_:person-beatriz-esteves a dct:Agent,
        foaf:Person ;
    scoro:hasORCID "0000-0003-0259-7560" ;
    org:memberOf _:org-idlab-imec-ghent-university ;
    foaf:homepage "https://w3id.org/people/besteves" ;
    foaf:name "Beatriz Esteves" .

