@prefix ai: <https://w3id.org/dpv/ai#> .
@prefix bibo: <http://purl.org/ontology/bibo/> .
@prefix dcam: <http://purl.org/dc/dcam/> .
@prefix dct: <http://purl.org/dc/terms/> .
@prefix dpv: <https://w3id.org/dpv#> .
@prefix eu-aiact: <https://w3id.org/dpv/legal/eu/aiact#> .
@prefix foaf: <http://xmlns.com/foaf/0.1/> .
@prefix org: <http://www.w3.org/ns/org#> .
@prefix owl: <http://www.w3.org/2002/07/owl#> .
@prefix pd: <https://w3id.org/dpv/pd#> .
@prefix profile: <http://www.w3.org/ns/dx/prof/> .
@prefix rdf: <http://www.w3.org/1999/02/22-rdf-syntax-ns#> .
@prefix rdfs: <http://www.w3.org/2000/01/rdf-schema#> .
@prefix risk: <https://w3id.org/dpv/risk#> .
@prefix role: <http://www.w3.org/ns/dx/prof/role/> .
@prefix schema: <https://schema.org/> .
@prefix scoro: <http://purl.org/spar/scoro/> .
@prefix skos: <http://www.w3.org/2004/02/skos/core#> .
@prefix sw: <http://www.w3.org/2003/06/sw-vocab-status/ns#> .
@prefix tech: <https://w3id.org/dpv/tech#> .
@prefix vann: <http://purl.org/vocab/vann/> .
@prefix xsd: <http://www.w3.org/2001/XMLSchema#> .

eu-aiact:AIActComplianceUnknown a rdfs:Class,
        skos:Concept,
        dpv:Lawfulness ;
    dct:contributor _:person-beatriz-esteves,
        _:person-harshvardhan-j-pandit ;
    dct:created "2024-07-21"^^xsd:date ;
    rdfs:isDefinedBy eu-aiact: ;
    sw:term_status "accepted"@en ;
    skos:broader eu-aiact:AIActLawfulness ;
    skos:definition "State where lawfulness or compliance with AI Act is unknown"@en ;
    skos:inScheme eu-aiact:compliance-classes ;
    skos:prefLabel "AI Act Compliance Unknown"@en .

eu-aiact:AIActCompliant a rdfs:Class,
        skos:Concept,
        dpv:Lawfulness ;
    dct:contributor _:person-beatriz-esteves,
        _:person-harshvardhan-j-pandit ;
    dct:created "2024-07-21"^^xsd:date ;
    rdfs:isDefinedBy eu-aiact: ;
    sw:term_status "accepted"@en ;
    skos:broader eu-aiact:AIActLawfulness ;
    skos:definition "State of being lawful or legally compliant for AI Act"@en ;
    skos:inScheme eu-aiact:compliance-classes ;
    skos:prefLabel "AI Act Compliant"@en .

eu-aiact:AIActLawfulness a rdfs:Class,
        skos:Concept,
        dpv:Lawfulness ;
    dct:contributor _:person-beatriz-esteves,
        _:person-harshvardhan-j-pandit ;
    dct:created "2024-07-21"^^xsd:date ;
    rdfs:isDefinedBy eu-aiact: ;
    sw:term_status "accepted"@en ;
    skos:broader dpv:Lawfulness ;
    skos:definition "Status or state associated with being lawful or legally compliant regarding AI Act"@en ;
    skos:inScheme eu-aiact:compliance-classes ;
    skos:prefLabel "AI Act Lawfulness"@en .

eu-aiact:AIActNonCompliant a rdfs:Class,
        skos:Concept,
        dpv:Lawfulness ;
    dct:contributor _:person-beatriz-esteves,
        _:person-harshvardhan-j-pandit ;
    dct:created "2024-07-21"^^xsd:date ;
    rdfs:isDefinedBy eu-aiact: ;
    sw:term_status "accepted"@en ;
    skos:broader eu-aiact:AIActLawfulness ;
    skos:definition "State of being unlawful or legally non-compliant for AI Act"@en ;
    skos:inScheme eu-aiact:compliance-classes ;
    skos:prefLabel "AI Act Non-compliant"@en .

eu-aiact:AIDeployer a rdfs:Class,
        skos:Concept ;
    dct:contributor _:person-delaram-golpayegani ;
    dct:created "2024-04-10"^^xsd:date ;
    dct:modified "2025-07-30"^^xsd:date ;
    dct:source "AIA (Art. 3(4))"@en ;
    rdfs:isDefinedBy eu-aiact: ;
    rdfs:subClassOf eu-aiact:AIOperator,
        tech:Deployer ;
    sw:term_status "modified"@en ;
    skos:broader eu-aiact:AIOperator,
        tech:Deployer ;
    skos:definition "A natural or legal person, public authority, agency or other body using an AI system under its authority except where the AI system is used in the course of a personal non-professional activity"@en ;
    skos:inScheme eu-aiact:roles-classes ;
    skos:prefLabel "AI Deployer"@en .

eu-aiact:AIDistributor a rdfs:Class,
        skos:Concept ;
    dct:contributor _:person-delaram-golpayegani ;
    dct:created "2024-04-10"^^xsd:date ;
    dct:source "AIA (Art. 3(7))"@en ;
    rdfs:isDefinedBy eu-aiact: ;
    rdfs:subClassOf eu-aiact:AIOperator,
        tech:Distributor ;
    sw:term_status "accepted"@en ;
    skos:broader eu-aiact:AIOperator,
        tech:Distributor ;
    skos:definition "A natural or legal person in the supply chain, other than the provider or the importer, that makes an AI system available on the Union market"@en ;
    skos:inScheme eu-aiact:roles-classes ;
    skos:prefLabel "AI Distributor"@en .

eu-aiact:AIImporter a rdfs:Class,
        skos:Concept ;
    dct:contributor _:person-delaram-golpayegani ;
    dct:created "2024-04-10"^^xsd:date ;
    dct:modified "2025-07-30"^^xsd:date ;
    dct:source "AIA (Art. 3(6))"@en ;
    rdfs:isDefinedBy eu-aiact: ;
    rdfs:subClassOf eu-aiact:AIOperator,
        tech:Importer ;
    sw:term_status "modified"@en ;
    skos:broader eu-aiact:AIOperator,
        tech:Importer ;
    skos:definition "A natural or legal person located or established in the Union that places on the market an AI system that bears the name or trademark of a natural or legal person established in a third country"@en ;
    skos:inScheme eu-aiact:roles-classes ;
    skos:prefLabel "AI Importer"@en .

eu-aiact:AILiteracy a rdfs:Class,
        skos:Concept,
        dpv:OrganisationalMeasure ;
    dct:contributor _:person-delaram-golpayegani ;
    dct:created "2024-04-10"^^xsd:date ;
    dct:modified "2025-07-30"^^xsd:date ;
    dct:source "AIA (Art. 3(56))"@en ;
    rdfs:isDefinedBy eu-aiact: ;
    sw:term_status "modified"@en ;
    skos:broader dpv:AILiteracy ;
    skos:definition "Skills, knowledge and understanding that allow providers, deployers and affected persons, taking into account their respective rights and obligations in the context of this Regulation, to make an informed deployment of AI systems, as well as to gain awareness about the opportunities and risks of AI and possible harm it can cause"@en ;
    skos:inScheme eu-aiact:misc-classes ;
    skos:prefLabel "AI Literacy"@en .

eu-aiact:AIOffice a rdfs:Class,
        skos:Concept ;
    dct:contributor _:person-delaram-golpayegani ;
    dct:created "2024-04-10"^^xsd:date ;
    dct:modified "2027-07-30"^^xsd:date ;
    dct:source "AIA(Art. 3(47))"@en ;
    rdfs:isDefinedBy eu-aiact: ;
    rdfs:subClassOf dpv:Authority ;
    sw:term_status "modified"@en ;
    skos:broader dpv:Authority ;
    skos:definition "the Commission’s function of contributing to the implementation, monitoring and supervision of AI systems and general-purpose AI models, and AI governance, provided for in Commission Decision of 24 January 2024; references in the AI Act to the AI Office shall be construed as references to the Commission"@en ;
    skos:inScheme eu-aiact:roles-classes ;
    skos:prefLabel "Artificial Intelligence Office"@en .

eu-aiact:AIOperator a rdfs:Class,
        skos:Concept ;
    dct:contributor _:person-delaram-golpayegani ;
    dct:created "2024-04-10"^^xsd:date ;
    dct:modified "2025-07-30"^^xsd:date ;
    dct:source "AIA (Art. 3(8))"@en ;
    rdfs:isDefinedBy eu-aiact: ;
    rdfs:subClassOf tech:Operator ;
    sw:term_status "modified"@en ;
    skos:broader tech:Operator ;
    skos:definition "A provider, product manufacturer, deployer, authorised representative, importer or distributor"@en ;
    skos:inScheme eu-aiact:roles-classes ;
    skos:prefLabel "AI Operator"@en .

eu-aiact:AIProductManufacturer a rdfs:Class,
        skos:Concept ;
    dct:contributor _:person-delaram-golpayegani ;
    dct:created "2024-04-10"^^xsd:date ;
    dct:modified "2027-07-30"^^xsd:date ;
    rdfs:isDefinedBy eu-aiact: ;
    rdfs:subClassOf eu-aiact:AIOperator,
        tech:Manufacturer ;
    sw:term_status "modified"@en ;
    skos:broader eu-aiact:AIOperator,
        tech:Manufacturer ;
    skos:definition "Entity that manufactures an AI Product"@en ;
    skos:inScheme eu-aiact:roles-classes ;
    skos:prefLabel "AI Product Manufacturer"@en .

eu-aiact:AIProvider a rdfs:Class,
        skos:Concept ;
    dct:contributor _:person-delaram-golpayegani ;
    dct:created "2024-04-10"^^xsd:date ;
    dct:modified "2025-07-30"^^xsd:date ;
    dct:source "AIA (Art. 3(3))"@en ;
    rdfs:isDefinedBy eu-aiact: ;
    rdfs:subClassOf eu-aiact:AIOperator,
        tech:Provider ;
    sw:term_status "modified"@en ;
    skos:broader eu-aiact:AIOperator,
        tech:Provider ;
    skos:definition "A natural or legal person, public authority, agency or other body that develops an AI system or a general-purpose AI model or that has an AI system or a general-purpose AI model developed and places it on the market or puts the AI system into service under its own name or trademark, whether for payment or free of charge"@en ;
    skos:inScheme eu-aiact:roles-classes ;
    skos:prefLabel "AI Provider"@en .

eu-aiact:AIRegulatorySandbox a rdfs:Class,
        skos:Concept,
        dpv:OrganisationalMeasure ;
    dct:contributor _:person-delaram-golpayegani ;
    dct:created "2024-04-10"^^xsd:date ;
    dct:modified "2024-07-30"^^xsd:date ;
    dct:source "AIA (Art. 3(55))"@en ;
    rdfs:isDefinedBy eu-aiact: ;
    sw:term_status "modified"@en ;
    skos:broader dpv:RegulatorySandbox ;
    skos:definition "A controlled framework set up by a competent authority which offers providers or prospective providers of AI systems the possibility to develop, train, validate and test, where appropriate in real-world conditions, an innovative AI system, pursuant to a sandbox plan for a limited time under regulatory supervision"@en ;
    skos:inScheme eu-aiact:assessment-classes ;
    skos:prefLabel "AI Regulatory Sandbox"@en .

eu-aiact:AISystem a rdfs:Class,
        skos:Concept ;
    dct:contributor _:person-delaram-golpayegani ;
    dct:created "2024-04-10"^^xsd:date ;
    dct:source "AIA (Art. 3(1))"@en ;
    rdfs:isDefinedBy eu-aiact: ;
    rdfs:subClassOf ai:AISystem ;
    sw:term_status "accepted"@en ;
    skos:broader ai:AISystem ;
    skos:definition "A machine-based system designed to operate with varying levels of autonomy and that may exhibit adaptiveness after deployment and that, for explicit or implicit objectives, infers, from the input it receives, how to generate outputs such as predictions, content, recommendations, or decisions that can influence physical or virtual environments."@en ;
    skos:inScheme eu-aiact:system-classes ;
    skos:prefLabel "AI System"@en ;
    skos:scopeNote "Note All references to the AI Act referred to the provisional agreement published in Feb 2024"@en .

eu-aiact:AISystemPerformance a rdfs:Class,
        skos:Concept ;
    dct:contributor _:person-delaram-golpayegani ;
    dct:created "2024-04-10"^^xsd:date ;
    dct:source "AIA(Art. 3(18))"@en ;
    rdfs:isDefinedBy eu-aiact: ;
    sw:term_status "accepted"@en ;
    skos:definition "The ability of an AI system to achieve its intended purpose"@en ;
    skos:inScheme eu-aiact:assessment-classes ;
    skos:prefLabel "AI System Performance"@en .

eu-aiact:AsylumSector a rdfs:Class,
        skos:Concept,
        dpv:Sector ;
    dct:contributor _:person-delaram-golpayegani,
        _:person-harshvardhan-j-pandit ;
    dct:created "2024-12-01"^^xsd:date ;
    dct:source " Annex III"@en,
        "EU AI Act"@en ;
    rdfs:isDefinedBy eu-aiact: ;
    sw:term_status "accepted"@en ;
    skos:broader dpv:Sector ;
    skos:definition "Sector related to asylum management"@en ;
    skos:inScheme eu-aiact:sector-classes ;
    skos:prefLabel "Asylum Sector"@en .

eu-aiact:AuthorisedRepresentative a rdfs:Class,
        skos:Concept ;
    dct:contributor _:person-delaram-golpayegani ;
    dct:created "2024-04-10"^^xsd:date ;
    dct:source "AIA (Art. 3(5))"@en ;
    rdfs:isDefinedBy eu-aiact: ;
    rdfs:subClassOf dpv:Representative,
        eu-aiact:AIOperator ;
    sw:term_status "accepted"@en ;
    skos:broader dpv:Representative,
        eu-aiact:AIOperator ;
    skos:definition "A natural or legal person located or established in the Union who has received and accepted a written mandate from a provider of an AI system or a general-purpose AI model to, respectively, perform and carry out on its behalf the obligations and procedures established by the AI Act"@en ;
    skos:inScheme eu-aiact:roles-classes ;
    skos:prefLabel "Authorised Representative"@en .

eu-aiact:AvailableOnEUMarket a rdfs:Class,
        skos:Concept,
        eu-aiact:MarketAvailabilityStatus ;
    dct:contributor _:person-delaram-golpayegani ;
    dct:created "2024-05-17"^^xsd:date ;
    dct:source "AIA (Art. 3(10))"@en ;
    rdfs:isDefinedBy eu-aiact: ;
    sw:term_status "accepted"@en ;
    skos:broader eu-aiact:AvailableOnMarket ;
    skos:definition "Status associated with supply of an AI system or a general purpose AI model for distribution or use on the Union market in the course of a commercial activity, whether in return for payment or free of charge"@en ;
    skos:inScheme eu-aiact:status-classes ;
    skos:prefLabel "Available on EU Market"@en .

eu-aiact:AvailableOnMarket a rdfs:Class,
        skos:Concept,
        eu-aiact:MarketAvailabilityStatus ;
    dct:contributor _:person-delaram-golpayegani ;
    dct:created "2024-05-17"^^xsd:date ;
    dct:source "AIA (Art. 3(10))"@en ;
    rdfs:isDefinedBy eu-aiact: ;
    sw:term_status "accepted"@en ;
    skos:broader eu-aiact:MarketAvailabilityStatus ;
    skos:definition "Status associated with supply of an AI system or a general purpose AI model for distribution or use on the market in the course of a commercial activity, whether in return for payment or free of charge"@en ;
    skos:inScheme eu-aiact:status-classes ;
    skos:prefLabel "Available on Market"@en .

eu-aiact:AvailableOnNonEUMarket a rdfs:Class,
        skos:Concept,
        eu-aiact:MarketAvailabilityStatus ;
    dct:contributor _:person-delaram-golpayegani ;
    dct:created "2024-05-17"^^xsd:date ;
    rdfs:isDefinedBy eu-aiact: ;
    sw:term_status "accepted"@en ;
    skos:broader eu-aiact:AvailableOnMarket ;
    skos:definition "Status associated with supply of an AI system or a general purpose AI model for distribution or use on any market except the Union market in the course of a commercial activity, whether in return for payment or free of charge"@en ;
    skos:inScheme eu-aiact:status-classes ;
    skos:prefLabel "Available on Non-EU Market"@en .

eu-aiact:BiometricCategorisation a rdfs:Class,
        skos:Concept,
        tech:Capability ;
    dct:contributor _:person-delaram-golpayegani ;
    dct:created "2024-04-10"^^xsd:date ;
    dct:modified "2025-07-30"^^xsd:date ;
    dct:source "AIA Art. 3(40)"@en ;
    rdfs:isDefinedBy eu-aiact: ;
    sw:term_status "modified"@en ;
    skos:broader ai:BiometricCategorisation ;
    skos:definition "Capability where assigning natural persons to specific categories happens on the basis of their biometric data unless ancillary to another commercial service and strictly necessary for objective technical reasons"@en ;
    skos:inScheme eu-aiact:capability-classes ;
    skos:prefLabel "Biometric Categorisation"@en ;
    skos:related pd:Biometric .

eu-aiact:BiometricCategorisationSystem a rdfs:Class,
        skos:Concept,
        eu-aiact:AISystem ;
    dct:contributor _:person-delaram-golpayegani ;
    dct:created "2024-04-10"^^xsd:date ;
    dct:modified "2025-07-30"^^xsd:date ;
    dct:source "AIA(Art. 3(40))"@en ;
    rdfs:isDefinedBy eu-aiact: ;
    sw:term_status "modified"@en ;
    skos:broader eu-aiact:AISystem ;
    skos:definition "An AI system for the purpose of assigning natural persons to specific categories on the basis of their biometric data, unless it is ancillary to another commercial service and strictly necessary for objective technical reasons"@en ;
    skos:inScheme eu-aiact:system-classes ;
    skos:prefLabel "Biometric Categorisation System"@en ;
    skos:related pd:Biometric .

eu-aiact:BiometricData a rdfs:Class,
        skos:Concept,
        dpv:PersonalData ;
    dct:contributor _:person-delaram-golpayegani ;
    dct:created "2024-04-10"^^xsd:date ;
    dct:modified "2025-07-30"^^xsd:date ;
    dct:source "AIA(Art. 3(34))"@en ;
    rdfs:isDefinedBy eu-aiact: ;
    sw:term_status "accepted"@en ;
    skos:broader pd:Biometric ;
    skos:definition "Personal data resulting from specific technical processing relating to the physical, physiological or behavioural characteristics of a natural person, such as facial images or dactyloscopic data"@en ;
    skos:inScheme eu-aiact:data-classes ;
    skos:prefLabel "Biometric Data"@en .

eu-aiact:BiometricIdentification a rdfs:Class,
        skos:Concept,
        tech:Capability ;
    dct:contributor _:person-delaram-golpayegani ;
    dct:created "2024-04-10"^^xsd:date ;
    dct:modified "2025-07-30"^^xsd:date ;
    dct:source "AIA Art. 3(35)"@en ;
    rdfs:isDefinedBy eu-aiact: ;
    sw:term_status "modified"@en ;
    skos:broader ai:BiometricIdentification ;
    skos:definition "Capability where the automated recognition of physical, physiological, behavioural, and psychological human features are used for the purpose of establishing the identity of a natural person by comparing biometric data of that individual to to biometric data of individuals stored in a database"@en ;
    skos:inScheme eu-aiact:capability-classes ;
    skos:prefLabel "Biometric Identification"@en ;
    skos:related pd:Biometric .

eu-aiact:BiometricVerification a rdfs:Class,
        skos:Concept,
        tech:Capability ;
    dct:contributor _:person-delaram-golpayegani ;
    dct:created "2024-04-10"^^xsd:date ;
    dct:modified "2025-07-30"^^xsd:date ;
    dct:source "AIA Art.3 (36)"@en ;
    rdfs:isDefinedBy eu-aiact: ;
    sw:term_status "modified"@en ;
    skos:broader dpv:IdentityVerification ;
    skos:definition "The automated, one-to-one verification, including authentication, of the identity of natural persons by comparing their biometric data to previously provided biometric data"@en ;
    skos:inScheme eu-aiact:capability-classes ;
    skos:prefLabel "Biometric Verification"@en ;
    skos:related pd:Biometric .

eu-aiact:BorderControlSector a rdfs:Class,
        skos:Concept,
        dpv:Sector ;
    dct:contributor _:person-delaram-golpayegani,
        _:person-harshvardhan-j-pandit ;
    dct:created "2024-12-01"^^xsd:date ;
    dct:source " Annex III"@en,
        "EU AI Act"@en ;
    rdfs:isDefinedBy eu-aiact: ;
    sw:term_status "accepted"@en ;
    skos:broader dpv:Sector ;
    skos:definition "Sector related to border control management"@en ;
    skos:inScheme eu-aiact:sector-classes ;
    skos:prefLabel "Border Control Sector"@en .

eu-aiact:CEMarking a rdfs:Class,
        skos:Concept,
        dpv:OrganisationalMeasure ;
    dct:contributor _:person-delaram-golpayegani ;
    dct:created "2024-04-10"^^xsd:date ;
    dct:modified "2024-07-30"^^xsd:date ;
    dct:source "AIA(Art. 3(24))"@en ;
    rdfs:isDefinedBy eu-aiact: ;
    sw:term_status "modified"@en ;
    skos:broader dpv:CertificationSeal ;
    skos:definition "A marking by which a provider indicates that an AI system is in conformity with the requirements set out in Chapter III, Section 2 and other applicable Union harmonisation legislation providing for its affixing"@en ;
    skos:inScheme eu-aiact:assessment-classes ;
    skos:prefLabel "CE Marking"@en .

eu-aiact:ChangeCategory a rdfs:Class,
        skos:Concept ;
    dct:contributor _:person-delaram-golpayegani ;
    dct:created "2024-12-01"^^xsd:date ;
    rdfs:isDefinedBy eu-aiact: ;
    rdfs:subClassOf dpv:Context ;
    sw:term_status "accepted"@en ;
    skos:broader dpv:Context ;
    skos:definition "A categorisation of the change associated with the AI system"@en ;
    skos:inScheme eu-aiact:status-classes ;
    skos:prefLabel "Change Category"@en .

eu-aiact:ChangeDescription a rdfs:Class,
        skos:Concept ;
    dct:contributor _:person-delaram-golpayegani ;
    dct:created "2024-12-01"^^xsd:date ;
    rdfs:isDefinedBy eu-aiact: ;
    rdfs:subClassOf dpv:Context ;
    sw:term_status "accepted"@en ;
    skos:broader dpv:Context ;
    skos:definition "A description of the change associated with the AI system"@en ;
    skos:inScheme eu-aiact:status-classes ;
    skos:prefLabel "Change Description"@en .

eu-aiact:CommonSpecification a rdfs:Class,
        skos:Concept,
        tech:Documentation ;
    dct:contributor _:person-delaram-golpayegani ;
    dct:created "2024-04-10"^^xsd:date ;
    dct:modified "2024-12-17"^^xsd:date ;
    dct:source "AIA Art.3-28"@en ;
    rdfs:isDefinedBy eu-aiact: ;
    sw:term_status "modified"@en ;
    skos:broader tech:Specification ;
    skos:definition "A set of technical specifications, as defined in point 4 of Article 2 of Regulation (EU) No 1025/2012 providing means to comply with certain requirements established under the AI Act"@en ;
    skos:inScheme eu-aiact:docs-classes ;
    skos:prefLabel "Common Specification"@en .

eu-aiact:ConformityAssessment a rdfs:Class,
        skos:Concept,
        dpv:OrganisationalMeasure ;
    dct:contributor _:person-delaram-golpayegani ;
    dct:created "2024-04-10"^^xsd:date ;
    dct:modified "2024-07-30"^^xsd:date ;
    dct:source "AIA(Art. 3(20))"@en ;
    rdfs:isDefinedBy eu-aiact: ;
    sw:term_status "modified"@en ;
    skos:broader dpv:Assessment ;
    skos:definition "The process of demonstrating whether the requirements set out in Chapter III, Section 2 relating to a high-risk AI system have been fulfilled"@en ;
    skos:inScheme eu-aiact:assessment-classes ;
    skos:prefLabel "Conformity Assessment"@en .

eu-aiact:ConformityAssessmentBody a rdfs:Class,
        skos:Concept ;
    dct:contributor _:person-delaram-golpayegani ;
    dct:created "2024-04-10"^^xsd:date ;
    dct:source "AIA(Art. 3(21))"@en ;
    rdfs:isDefinedBy eu-aiact: ;
    rdfs:subClassOf tech:Auditor ;
    sw:term_status "accepted"@en ;
    skos:broader tech:Auditor ;
    skos:definition "A body that performs third-party conformity assessment activities, including testing, certification and inspection"@en ;
    skos:inScheme eu-aiact:roles-classes ;
    skos:prefLabel "Conformity Assessment Body"@en .

eu-aiact:CriticalInfrastructureSector a rdfs:Class,
        skos:Concept,
        dpv:Sector ;
    dct:contributor _:person-delaram-golpayegani,
        _:person-harshvardhan-j-pandit ;
    dct:created "2024-12-01"^^xsd:date ;
    dct:source " Annex III"@en,
        "EU AI Act"@en ;
    rdfs:isDefinedBy eu-aiact: ;
    sw:term_status "accepted"@en ;
    skos:broader dpv:Sector ;
    skos:definition "Sector related to provision and maintenance of critical services"@en ;
    skos:inScheme eu-aiact:sector-classes ;
    skos:prefLabel "Critical Infrastructure Sector"@en .

eu-aiact:DeepFakeGeneration a rdfs:Class,
        skos:Concept,
        tech:Capability ;
    dct:contributor _:person-delaram-golpayegani ;
    dct:created "2024-04-10"^^xsd:date ;
    dct:modified "2025-07-30"^^xsd:date ;
    dct:source "AIA Art. 3(60)"@en ;
    rdfs:isDefinedBy eu-aiact: ;
    sw:term_status "modified"@en ;
    skos:broader ai:BiometricIdentification ;
    skos:definition "Capability to generate or manipulate image, audio or video content that resembles existing persons, objects, places, entities or events and would falsely appear to a person to be authentic or truthful;l"@en ;
    skos:inScheme eu-aiact:capability-classes ;
    skos:prefLabel "Deep Fake Generation"@en .

eu-aiact:DemocraticProcessSector a rdfs:Class,
        skos:Concept,
        dpv:Sector ;
    dct:contributor _:person-delaram-golpayegani,
        _:person-harshvardhan-j-pandit ;
    dct:created "2024-12-01"^^xsd:date ;
    dct:source " Annex III"@en,
        "EU AI Act"@en ;
    rdfs:isDefinedBy eu-aiact: ;
    sw:term_status "accepted"@en ;
    skos:broader dpv:Sector ;
    skos:definition "Sector related to administration of democratic processes"@en ;
    skos:inScheme eu-aiact:sector-classes ;
    skos:prefLabel "Democratic Process Sector"@en .

eu-aiact:DownstreamAIProvider a rdfs:Class,
        skos:Concept ;
    dct:contributor _:person-delaram-golpayegani ;
    dct:created "2024-04-10"^^xsd:date ;
    dct:modified "2025-07-30"^^xsd:date ;
    dct:source "AIA(Art. 3(68))"@en ;
    rdfs:isDefinedBy eu-aiact: ;
    rdfs:subClassOf eu-aiact:AIProvider ;
    sw:term_status "accepted"@en ;
    skos:broader eu-aiact:AIProvider ;
    skos:definition "A provider of an AI system, including a general-purpose AI system, which integrates an AI model, regardless of whether the AI model is provided by themselves and vertically integrated or provided by another entity based on contractual relations."@en ;
    skos:inScheme eu-aiact:roles-classes ;
    skos:prefLabel "Downstream AI Provider"@en .

eu-aiact:EUDeclarationOfConformity a rdfs:Class,
        skos:Concept,
        tech:Documentation ;
    dct:contributor _:person-delaram-golpayegani ;
    dct:created "2024-12-01"^^xsd:date ;
    dct:source "AI Act Art.47"@en ;
    rdfs:isDefinedBy eu-aiact: ;
    sw:term_status "accepted"@en ;
    skos:broader tech:Documentation ;
    skos:definition "Document providing the EU declaration of conformity, as required by the AI Act, Article 47"@en ;
    skos:inScheme eu-aiact:docs-classes ;
    skos:prefLabel "EU Declaration Of Conformity"@en .

eu-aiact:EducationSector a rdfs:Class,
        skos:Concept,
        dpv:Sector ;
    dct:contributor _:person-delaram-golpayegani,
        _:person-harshvardhan-j-pandit ;
    dct:created "2024-12-01"^^xsd:date ;
    dct:source " Annex III"@en,
        "EU AI Act"@en ;
    rdfs:isDefinedBy eu-aiact: ;
    sw:term_status "accepted"@en ;
    skos:broader dpv:Sector ;
    skos:definition "Sector related to education and vocational training at any level and for any profession"@en ;
    skos:inScheme eu-aiact:sector-classes ;
    skos:prefLabel "Education Sector"@en .

eu-aiact:EmotionRecognition a rdfs:Class,
        skos:Concept,
        tech:Capability ;
    dct:contributor _:person-delaram-golpayegani ;
    dct:created "2024-04-10"^^xsd:date ;
    dct:modified "2025-07-30"^^xsd:date ;
    dct:source "AIA Art. 3(39)"@en ;
    rdfs:isDefinedBy eu-aiact: ;
    sw:term_status "modified"@en ;
    skos:broader ai:EmotionRecognition ;
    skos:definition "Capability of a technology to identify or infer emotions or intentions of natural persons (on the basis of their biometric data)"@en ;
    skos:inScheme eu-aiact:capability-classes ;
    skos:prefLabel "Emotion Recognition"@en ;
    skos:related pd:Biometric .

eu-aiact:EmotionRecognitionSystem a rdfs:Class,
        skos:Concept,
        eu-aiact:AISystem ;
    dct:contributor _:person-delaram-golpayegani ;
    dct:created "2024-04-10"^^xsd:date ;
    dct:modified "2025-07-30"^^xsd:date ;
    dct:source "AIA(Art. 3(39))"@en ;
    rdfs:isDefinedBy eu-aiact: ;
    sw:term_status "modified"@en ;
    skos:broader eu-aiact:AISystem ;
    skos:definition "An AI system for the purpose of identifying or inferring emotions or intentions of natural persons on the basis of their biometric data."@en ;
    skos:inScheme eu-aiact:system-classes ;
    skos:prefLabel "Emotion Recognition System"@en ;
    skos:related eu-aiact:EmotionRecognition,
        pd:Biometric .

eu-aiact:EmploymentSector a rdfs:Class,
        skos:Concept,
        dpv:Sector ;
    dct:contributor _:person-delaram-golpayegani,
        _:person-harshvardhan-j-pandit ;
    dct:created "2024-12-01"^^xsd:date ;
    dct:source " Annex III"@en,
        "EU AI Act"@en ;
    rdfs:isDefinedBy eu-aiact: ;
    sw:term_status "accepted"@en ;
    skos:broader dpv:Sector ;
    skos:definition "Sector related to employment including workforce management and self-employment"@en ;
    skos:inScheme eu-aiact:sector-classes ;
    skos:prefLabel "Employment Sector"@en .

eu-aiact:FRIA a rdfs:Class,
        skos:Concept,
        dpv:OrganisationalMeasure ;
    dct:contributor _:person-delaram-golpayegani ;
    dct:created "2024-04-10"^^xsd:date ;
    dct:modified "2024-07-30"^^xsd:date ;
    dct:source "AIA(Art. 27)"@en ;
    rdfs:isDefinedBy eu-aiact: ;
    sw:term_status "modified"@en ;
    skos:broader dpv:Assessment ;
    skos:definition "An assessment undertaken to evaluate how the AI use of an AI system might impact fundamental rights"@en ;
    skos:inScheme eu-aiact:assessment-classes ;
    skos:prefLabel "Fundamental Rights Impact Assessment"@en .

eu-aiact:GPAIModel a rdfs:Class,
        skos:Concept ;
    dct:contributor _:person-delaram-golpayegani ;
    dct:created "2024-04-10"^^xsd:date ;
    dct:modified "2025-07-30"^^xsd:date ;
    dct:source "AIA(Art. 3(63))"@en ;
    rdfs:isDefinedBy eu-aiact: ;
    rdfs:subClassOf ai:Model ;
    sw:term_status "modified"@en ;
    skos:broader ai:Model ;
    skos:definition "An AI model, including where such an AI model is trained with a large amount of data using self-supervision at scale, that displays significant generality and is capable of competently performing a wide range of distinct tasks regardless of the way the model is placed on the market and that can be integrated into a variety of downstream systems or applications, except AI models that are used for research, development or prototyping activities before they are placed on the market"@en ;
    skos:inScheme eu-aiact:system-classes ;
    skos:prefLabel "General Purpose AI Model"@en .

eu-aiact:GPAISystem a rdfs:Class,
        skos:Concept ;
    dct:contributor _:person-delaram-golpayegani ;
    dct:created "2024-04-10"^^xsd:date ;
    dct:modified "2025-07-30"^^xsd:date ;
    dct:source "AIA(Art.3 (66))"@en ;
    rdfs:isDefinedBy eu-aiact: ;
    rdfs:subClassOf eu-aiact:AISystem ;
    sw:term_status "modified"@en ;
    skos:broader eu-aiact:AISystem ;
    skos:definition "An AI system which is based on a general-purpose AI model and which has the capability to serve a variety of purposes, both for direct use as well as for integration in other AI systems"@en ;
    skos:inScheme eu-aiact:system-classes ;
    skos:prefLabel "General Purpose AI System"@en .

eu-aiact:HighImpactCapabilityGPAIModel a rdfs:Class,
        skos:Concept,
        tech:Capability ;
    dct:contributor _:person-delaram-golpayegani ;
    dct:created "2024-04-10"^^xsd:date ;
    dct:modified "2025-07-30"^^xsd:date ;
    dct:source "AIA Art. 3(64)"@en ;
    rdfs:isDefinedBy eu-aiact: ;
    sw:term_status "modified"@en ;
    skos:broader tech:Capability ;
    skos:definition "‘High-impact Capabilities’ in general purpose AI models means capabilities that match or exceed the capabilities recorded in the most  advanced general purpose AI models"@en ;
    skos:inScheme eu-aiact:capability-classes ;
    skos:prefLabel "High-Impact Capability in General Purpose AI Models"@en .

eu-aiact:HighRiskAIAssessment a rdfs:Class,
        skos:Concept,
        dpv:OrganisationalMeasure ;
    dct:contributor _:person-delaram-golpayegani ;
    dct:created "2024-04-10"^^xsd:date ;
    dct:modified "2024-07-30"^^xsd:date ;
    dct:source "AIA(Art. 6)"@en ;
    rdfs:isDefinedBy eu-aiact: ;
    sw:term_status "modified"@en ;
    skos:broader dpv:Assessment ;
    skos:definition "An assessment undertaken to determine whether the AI system is classified as high-risk under the AI Act"@en ;
    skos:inScheme eu-aiact:assessment-classes ;
    skos:prefLabel "High Risk AI Assessment"@en .

eu-aiact:InformedConsent a rdfs:Class,
        skos:Concept,
        dpv:LegalBasis ;
    dct:contributor _:person-delaram-golpayegani ;
    dct:created "2024-04-10"^^xsd:date ;
    dct:modified "2024-07-30"^^xsd:date ;
    dct:source "AIA (Art. 3(59))"@en ;
    rdfs:isDefinedBy eu-aiact: ;
    sw:term_status "modified"@en ;
    skos:broader dpv:InformedConsent ;
    skos:definition "Informed consent means a (real world test) subject’s freely given, specific, unambiguous and voluntary expression of his or her willingness to participate in a particular testing in real world conditions, after having been informed of all aspects of the testing that are relevant to the subject’s decision to participate"@en ;
    skos:inScheme eu-aiact:assessment-classes ;
    skos:prefLabel "Informed Consent"@en .

eu-aiact:InstructionForUse a rdfs:Class,
        skos:Concept,
        tech:Documentation ;
    dct:contributor _:person-delaram-golpayegani ;
    dct:created "2024-04-10"^^xsd:date ;
    dct:modified "2025-07-31"^^xsd:date ;
    dct:source "AIA(Art.3(15))"@en ;
    rdfs:isDefinedBy eu-aiact: ;
    sw:term_status "modified"@en ;
    skos:broader tech:Instructions ;
    skos:definition "The information provided by the provider to inform the deployer of, in particular, an AI system’s intended purpose and proper use"@en ;
    skos:inScheme eu-aiact:docs-classes ;
    skos:prefLabel "Instruction For Use"@en .

eu-aiact:IntendedPurpose a rdfs:Class,
        skos:Concept ;
    dct:contributor _:person-delaram-golpayegani ;
    dct:created "2024-04-10"^^xsd:date ;
    dct:source "AIA (Art. 3(12))"@en ;
    rdfs:isDefinedBy eu-aiact: ;
    rdfs:subClassOf tech:IntendedUse ;
    sw:term_status "accepted"@en ;
    skos:broader tech:IntendedUse ;
    skos:definition "The use for which an AI system is intended by the provider, including the specific context and conditions of use, as specified in the information supplied by the provider in the instructions for use, promotional or sales materials and statements, as well as in the technical documentation"@en ;
    skos:inScheme eu-aiact:misc-classes ;
    skos:prefLabel "Intended Purpose"@en .

eu-aiact:JusticeSector a rdfs:Class,
        skos:Concept,
        dpv:Sector ;
    dct:contributor _:person-delaram-golpayegani,
        _:person-harshvardhan-j-pandit ;
    dct:created "2024-12-01"^^xsd:date ;
    dct:source " Annex III"@en,
        "EU AI Act"@en ;
    rdfs:isDefinedBy eu-aiact: ;
    sw:term_status "accepted"@en ;
    skos:broader dpv:Sector ;
    skos:definition "Sector related to administration of justice"@en ;
    skos:inScheme eu-aiact:sector-classes ;
    skos:prefLabel "Justice Sector"@en .

eu-aiact:LawEnforcementSector a rdfs:Class,
        skos:Concept,
        dpv:Sector ;
    dct:contributor _:person-delaram-golpayegani,
        _:person-harshvardhan-j-pandit ;
    dct:created "2024-12-01"^^xsd:date ;
    dct:source " Annex III"@en,
        "EU AI Act"@en ;
    rdfs:isDefinedBy eu-aiact: ;
    sw:term_status "accepted"@en ;
    skos:broader dpv:Sector ;
    skos:definition "Sector related to law enforcement"@en ;
    skos:inScheme eu-aiact:sector-classes ;
    skos:prefLabel "Law Enforcement Sector"@en .

eu-aiact:MarketAvailabilityStatus a rdfs:Class,
        skos:Concept ;
    dct:contributor _:person-delaram-golpayegani ;
    dct:created "2024-05-17"^^xsd:date ;
    rdfs:isDefinedBy eu-aiact: ;
    rdfs:subClassOf tech:MarketAvailabilityStatus ;
    sw:term_status "accepted"@en ;
    skos:broader tech:MarketAvailabilityStatus ;
    skos:definition "Status associated with whether the AI system or GPAI Model is available for distribution or use on the market in the course of a commercial activity"@en ;
    skos:inScheme eu-aiact:status-classes ;
    skos:prefLabel "Market Availability Status"@en .

eu-aiact:MarketPlacementStatus a rdfs:Class,
        skos:Concept ;
    dct:contributor _:person-delaram-golpayegani ;
    dct:created "2024-05-17"^^xsd:date ;
    rdfs:isDefinedBy eu-aiact: ;
    rdfs:subClassOf tech:MarketAvailabilityStatus ;
    sw:term_status "accepted"@en ;
    skos:broader tech:MarketAvailabilityStatus ;
    skos:definition "Status associated with whether the AI system or GPAI Model has been 'first' made available on the market"@en ;
    skos:inScheme eu-aiact:status-classes ;
    skos:prefLabel "Market Placement Status"@en .

eu-aiact:MarketSurveillanceAuthority a rdfs:Class,
        skos:Concept ;
    dct:contributor _:person-delaram-golpayegani ;
    dct:created "2024-04-10"^^xsd:date ;
    dct:source "AIA(Art. 3(26))"@en ;
    rdfs:isDefinedBy eu-aiact: ;
    rdfs:subClassOf eu-aiact:NationalCompetentAuthority ;
    sw:term_status "accepted"@en ;
    skos:broader eu-aiact:NationalCompetentAuthority ;
    skos:definition "The national authority carrying out the activities and taking the measures pursuant to Regulation (EU) 2019/1020"@en ;
    skos:inScheme eu-aiact:roles-classes ;
    skos:prefLabel "Market Surveillance Authority"@en .

eu-aiact:MigrationSector a rdfs:Class,
        skos:Concept,
        dpv:Sector ;
    dct:contributor _:person-delaram-golpayegani,
        _:person-harshvardhan-j-pandit ;
    dct:created "2024-12-01"^^xsd:date ;
    dct:source " Annex III"@en,
        "EU AI Act"@en ;
    rdfs:isDefinedBy eu-aiact: ;
    sw:term_status "accepted"@en ;
    skos:broader dpv:Sector ;
    skos:definition "Sector related to migration management"@en ;
    skos:inScheme eu-aiact:sector-classes ;
    skos:prefLabel "Migration Sector"@en .

eu-aiact:NationalCompetentAuthority a rdfs:Class,
        skos:Concept ;
    dct:contributor _:person-delaram-golpayegani ;
    dct:created "2024-04-10"^^xsd:date ;
    dct:modified "2027-07-30"^^xsd:date ;
    dct:source "AIA(Art. 3(48))"@en ;
    rdfs:isDefinedBy eu-aiact: ;
    rdfs:subClassOf dpv:Authority ;
    sw:term_status "modified"@en ;
    skos:broader dpv:Authority ;
    skos:definition "A notifying authority or a market surveillance authority; as regards AI systems put into service or used by Union institutions, agencies, offices and bodies, references to national competent authorities or market surveillance authorities in the AI Act shall be construed as references to the European Data Protection Supervisor"@en ;
    skos:inScheme eu-aiact:roles-classes ;
    skos:prefLabel "National Competent Authority"@en .

eu-aiact:NonpredeterminedChange a rdfs:Class,
        skos:Concept,
        eu-aiact:ChangeCategory ;
    dct:contributor _:person-delaram-golpayegani ;
    dct:created "2024-12-01"^^xsd:date ;
    rdfs:isDefinedBy eu-aiact: ;
    sw:term_status "accepted"@en ;
    skos:broader eu-aiact:ChangeCategory ;
    skos:definition "Change associated with the AI system that has not been pre-determined"@en ;
    skos:inScheme eu-aiact:status-classes ;
    skos:prefLabel "Non-Predetermined Change"@en ;
    skos:scopeNote "What is considered \"pre-determined\" is not defined with this concept or within the AI Act, therefore if there are specific interpretations of \"pre-determined\", such as within a jurisdiction, sector, or for a particular technology, then this concept should be extended accordingly"@en .

eu-aiact:NotAvailableOnMarket a rdfs:Class,
        skos:Concept,
        eu-aiact:MarketAvailabilityStatus ;
    dct:contributor _:person-delaram-golpayegani ;
    dct:created "2024-05-17"^^xsd:date ;
    rdfs:isDefinedBy eu-aiact: ;
    sw:term_status "accepted"@en ;
    skos:broader eu-aiact:MarketAvailabilityStatus ;
    skos:definition "not available on a market anywhere in EU or otherwise"@en ;
    skos:inScheme eu-aiact:status-classes ;
    skos:prefLabel "Not Available on Market"@en .

eu-aiact:NotPutIntoService a rdfs:Class,
        skos:Concept,
        eu-aiact:ServiceSupplyStatus ;
    dct:contributor _:person-delaram-golpayegani ;
    dct:created "2024-05-17"^^xsd:date ;
    rdfs:isDefinedBy eu-aiact: ;
    sw:term_status "accepted"@en ;
    skos:broader eu-aiact:ServiceSupplyStatus ;
    skos:definition "Status associated with an AI system that has not been put into service"@en ;
    skos:inScheme eu-aiact:status-classes ;
    skos:prefLabel "Not Put in to Service"@en .

eu-aiact:NotifiedBody a rdfs:Class,
        skos:Concept ;
    dct:contributor _:person-delaram-golpayegani ;
    dct:created "2024-04-10"^^xsd:date ;
    dct:source "AIA(Art. 3(22))"@en ;
    rdfs:isDefinedBy eu-aiact: ;
    rdfs:subClassOf eu-aiact:ConformityAssessmentBody ;
    sw:term_status "accepted"@en ;
    skos:broader eu-aiact:ConformityAssessmentBody ;
    skos:definition "A conformity assessment body notified in accordance with the AI Act and other relevant Union harmonisation legislation"@en ;
    skos:inScheme eu-aiact:roles-classes ;
    skos:prefLabel "Notified Body"@en .

eu-aiact:NotifyingAuthority a rdfs:Class,
        skos:Concept ;
    dct:contributor _:person-delaram-golpayegani ;
    dct:created "2024-04-10"^^xsd:date ;
    dct:source "AIA(Art. 3(19))"@en ;
    rdfs:isDefinedBy eu-aiact: ;
    rdfs:subClassOf eu-aiact:NationalCompetentAuthority ;
    sw:term_status "accepted"@en ;
    skos:broader eu-aiact:NationalCompetentAuthority ;
    skos:definition "The national authority responsible for setting up and carrying out the necessary procedures for the assessment, designation and notification of conformity assessment bodies and for their monitoring"@en ;
    skos:inScheme eu-aiact:roles-classes ;
    skos:prefLabel "Notifying Authority"@en .

eu-aiact:PlacedOnEUMarket a rdfs:Class,
        skos:Concept,
        eu-aiact:MarketPlacementStatus ;
    dct:contributor _:person-delaram-golpayegani ;
    dct:created "2024-05-17"^^xsd:date ;
    dct:source "AIA (Art. 3(9))"@en ;
    rdfs:isDefinedBy eu-aiact: ;
    sw:term_status "accepted"@en ;
    skos:broader eu-aiact:PlacedOnMarket ;
    skos:definition "Status indicating the first making available of an AI system or a general purpose AI model on the Union market"@en ;
    skos:inScheme eu-aiact:status-classes ;
    skos:prefLabel "Placed on EU Market"@en .

eu-aiact:PlacedOnMarket a rdfs:Class,
        skos:Concept,
        eu-aiact:MarketPlacementStatus ;
    dct:contributor _:person-delaram-golpayegani ;
    dct:created "2024-05-17"^^xsd:date ;
    dct:source "AIA (Art. 3(9))"@en ;
    rdfs:isDefinedBy eu-aiact: ;
    sw:term_status "accepted"@en ;
    skos:broader eu-aiact:MarketPlacementStatus ;
    skos:definition "Status indicating the first making available of an AI system or a general purpose AI model on the market"@en ;
    skos:inScheme eu-aiact:status-classes ;
    skos:prefLabel "Placed on Market"@en .

eu-aiact:PostMarketMonitoringPlan a rdfs:Class,
        skos:Concept,
        tech:Documentation ;
    dct:contributor _:person-delaram-golpayegani ;
    dct:created "2024-12-01"^^xsd:date ;
    dct:modified "2024-12-17"^^xsd:date ;
    dct:source "AI Act Art.72"@en ;
    rdfs:isDefinedBy eu-aiact: ;
    sw:term_status "modified"@en ;
    skos:broader tech:Plan ;
    skos:definition "Description of the post-market monitoring plan, as required by the AI Act"@en ;
    skos:inScheme eu-aiact:docs-classes ;
    skos:prefLabel "Post-market Monitoring Plan"@en .

eu-aiact:PostMarketMonitoringSystem a rdfs:Class,
        skos:Concept,
        dpv:OrganisationalMeasure ;
    dct:contributor _:person-delaram-golpayegani ;
    dct:created "2024-04-10"^^xsd:date ;
    dct:source "AIA(Art. 3(25))"@en ;
    rdfs:isDefinedBy eu-aiact: ;
    sw:term_status "accepted"@en ;
    skos:broader dpv:OrganisationalMeasure ;
    skos:definition """All activities carried out by providers of AI systems to collect and review experience gained from the use of AI systems they
place on the market or put into service for the purpose of identifying any need to immediately apply any necessary corrective or preventive actions"""@en ;
    skos:inScheme eu-aiact:assessment-classes ;
    skos:prefLabel "Post-Market Monitoring System"@en .

eu-aiact:PostMarketMonitoringSystemDocumentation a rdfs:Class,
        skos:Concept,
        tech:Documentation ;
    dct:contributor _:person-delaram-golpayegani ;
    dct:created "2024-12-01"^^xsd:date ;
    dct:source "AI Act Art.72"@en ;
    rdfs:isDefinedBy eu-aiact: ;
    sw:term_status "accepted"@en ;
    skos:broader tech:Documentation ;
    skos:definition "Documentation of the post-market monitoring system in place, as required by the AI Act"@en ;
    skos:inScheme eu-aiact:docs-classes ;
    skos:prefLabel "Post-market Monitoring System Documentation"@en .

eu-aiact:PostRemoteBiometricIdentificationSystem a rdfs:Class,
        skos:Concept,
        eu-aiact:AISystem ;
    dct:contributor _:person-delaram-golpayegani ;
    dct:created "2024-04-10"^^xsd:date ;
    dct:modified "2025-07-30"^^xsd:date ;
    dct:source "AIA(Art. 3(43))"@en ;
    rdfs:isDefinedBy eu-aiact: ;
    sw:term_status "modified"@en ;
    skos:broader eu-aiact:RemoteBiometricIdentificationSystem ;
    skos:definition "A remote biometric identification system other than a real-time remote biometric identification system"@en ;
    skos:inScheme eu-aiact:system-classes ;
    skos:prefLabel "Post Remote Biometric Identification System"@en ;
    skos:related pd:Biometric .

eu-aiact:PredeterminedChange a rdfs:Class,
        skos:Concept,
        eu-aiact:ChangeCategory ;
    dct:contributor _:person-delaram-golpayegani ;
    dct:created "2024-12-01"^^xsd:date ;
    rdfs:isDefinedBy eu-aiact: ;
    sw:term_status "accepted"@en ;
    skos:broader eu-aiact:ChangeCategory ;
    skos:definition "Change associated with the AI system that has been pre-determined"@en ;
    skos:inScheme eu-aiact:status-classes ;
    skos:prefLabel "Predetermined Change"@en ;
    skos:scopeNote "What is considered \"pre-determined\" is not defined with this concept or within the AI Act, therefore if there are specific interpretations of \"pre-determined\", such as within a jurisdiction, sector, or for a particular technology, then this concept should be extended accordingly"@en .

eu-aiact:PrivateSector a rdfs:Class,
        skos:Concept,
        dpv:Sector ;
    dct:contributor _:person-delaram-golpayegani,
        _:person-harshvardhan-j-pandit ;
    dct:created "2024-12-01"^^xsd:date ;
    dct:source " Annex III"@en,
        "EU AI Act"@en ;
    rdfs:isDefinedBy eu-aiact: ;
    sw:term_status "accepted"@en ;
    skos:broader dpv:Sector ;
    skos:definition "Sector comprising of entities that are privately owned"@en ;
    skos:inScheme eu-aiact:sector-classes ;
    skos:prefLabel "Private Sector"@en .

eu-aiact:PublicSector a rdfs:Class,
        skos:Concept,
        dpv:Sector ;
    dct:contributor _:person-delaram-golpayegani,
        _:person-harshvardhan-j-pandit ;
    dct:created "2024-12-01"^^xsd:date ;
    dct:source " Annex III"@en,
        "EU AI Act"@en ;
    rdfs:isDefinedBy eu-aiact: ;
    sw:term_status "accepted"@en ;
    skos:broader dpv:Sector ;
    skos:definition "Sector comprising of entities that are publicly owned e.g. by the government"@en ;
    skos:inScheme eu-aiact:sector-classes ;
    skos:prefLabel "Public Sector"@en .

eu-aiact:PubliclyAccessibleSpace a rdfs:Class,
        skos:Concept,
        dpv:Location ;
    dct:contributor _:person-delaram-golpayegani ;
    dct:created "2024-04-10"^^xsd:date ;
    dct:modified "2025-07-30"^^xsd:date ;
    dct:source "AIA(Art. 3(44))"@en ;
    rdfs:isDefinedBy eu-aiact: ;
    sw:term_status "modified"@en ;
    skos:broader dpv:PublicLocation ;
    skos:definition "Any publicly or privately owned physical place accessible to an undetermined number of natural persons, regardless of whether certain conditions for access may apply, and regardless of the potential capacity restrictions"@en ;
    skos:inScheme eu-aiact:misc-classes ;
    skos:prefLabel "Publicly Accessible Space"@en .

eu-aiact:PutIntoService a rdfs:Class,
        skos:Concept,
        eu-aiact:ServiceSupplyStatus ;
    dct:contributor _:person-delaram-golpayegani ;
    dct:created "2024-05-17"^^xsd:date ;
    dct:source "AIA (Art. 3(11))"@en ;
    rdfs:isDefinedBy eu-aiact: ;
    sw:term_status "accepted"@en ;
    skos:broader eu-aiact:ServiceSupplyStatus ;
    skos:definition "Status associated with the supply of an AI system for first use directly to the deployer or for own use for its intended purpose"@en ;
    skos:inScheme eu-aiact:status-classes ;
    skos:prefLabel "Put in to Service"@en .

eu-aiact:PutIntoServiceInEU a rdfs:Class,
        skos:Concept,
        eu-aiact:ServiceSupplyStatus ;
    dct:contributor _:person-delaram-golpayegani ;
    dct:created "2024-05-17"^^xsd:date ;
    dct:source "AIA (Art. 3(11))"@en ;
    rdfs:isDefinedBy eu-aiact: ;
    sw:term_status "accepted"@en ;
    skos:broader eu-aiact:PutIntoService ;
    skos:definition "Status associated with the supply of an AI system for first use directly to the deployer or for own use in the Union for its intended purpose"@en ;
    skos:inScheme eu-aiact:status-classes ;
    skos:prefLabel "Put in to Service In EU"@en .

eu-aiact:RealWorldTestSubject a rdfs:Class,
        skos:Concept ;
    dct:contributor _:person-delaram-golpayegani ;
    dct:created "2024-04-10"^^xsd:date ;
    dct:modified "2024-07-30"^^xsd:date ;
    dct:source "AIA (Art. 3(58))"@en ;
    rdfs:isDefinedBy eu-aiact: ;
    rdfs:subClassOf dpv:NaturalPerson ;
    sw:term_status "modified"@en ;
    skos:broader dpv:NaturalPerson ;
    skos:definition "A natural person who participates in testing in real world conditions"@en ;
    skos:inScheme eu-aiact:assessment-classes ;
    skos:prefLabel "Real World Test Subject"@en ;
    skos:scopeNote "Note: The term \"Real World Test Subject\" is defined as just \"Subject\" in the AI Act. We emphasise its distinction from other subjects, e.g. AI Subject, with this phrasing of the term."@en .

eu-aiact:RealWorldTestingPlan a rdfs:Class,
        skos:Concept,
        tech:Documentation ;
    dct:contributor _:person-delaram-golpayegani ;
    dct:created "2024-04-10"^^xsd:date ;
    dct:modified "2024-12-17"^^xsd:date ;
    dct:source "AIA Art.3-53"@en ;
    rdfs:isDefinedBy eu-aiact: ;
    sw:term_status "modified"@en ;
    skos:broader tech:Plan ;
    skos:definition "A document that describes the objectives, methodology, geographical, population and temporal scope, monitoring, organisation and conduct of testing in real world conditions."@en ;
    skos:inScheme eu-aiact:docs-classes ;
    skos:prefLabel "Real World Testing Plan"@en .

eu-aiact:RealtimeRemoteBiometricIdentificationSystem a rdfs:Class,
        skos:Concept,
        eu-aiact:AISystem ;
    dct:contributor _:person-delaram-golpayegani ;
    dct:created "2024-04-10"^^xsd:date ;
    dct:modified "2025-07-30"^^xsd:date ;
    dct:source "AIA(Art. 3(42))"@en ;
    rdfs:isDefinedBy eu-aiact: ;
    sw:term_status "modified"@en ;
    skos:broader eu-aiact:RemoteBiometricIdentificationSystem ;
    skos:definition "A remote biometric identification system, whereby the capturing of biometric data, the comparison and the identification all occur without a significant delay, comprising not only instant identification, but also limited short delays in order to avoid circumvention"@en ;
    skos:inScheme eu-aiact:system-classes ;
    skos:prefLabel "Real-time Remote Biometric Identification System"@en ;
    skos:related pd:Biometric .

eu-aiact:ReasonablyForeseeableMisuse a rdfs:Class,
        skos:Concept,
        dpv:RiskConcept ;
    dct:contributor _:person-arthit-suriyawongkul,
        _:person-delaram-golpayegani,
        _:person-georg-p-krog,
        _:person-harshvardhan-j-pandit ;
    dct:created "2024-04-10"^^xsd:date ;
    dct:modified "2025-06-19"^^xsd:date ;
    dct:source "AIA (Art. 3(13))"@en ;
    rdfs:isDefinedBy eu-aiact: ;
    sw:term_status "modified"@en ;
    skos:broader risk:Misuse ;
    skos:definition "The use of an AI system in a way that is not in accordance with its intended purpose, but which may result from reasonably foreseeable human behaviour or interaction with other systems, including other AI systems"@en ;
    skos:inScheme eu-aiact:misc-classes ;
    skos:prefLabel "Reasonably Foreseeable Misuse"@en ;
    skos:scopeNote "Misuse should be provided through the Risk extension, along with taxonomy e.g. Misuse -> Foreseeable -> Reasonably and NonReasonably Foreseeable; and Misuse -> Unforeseeable Misuse."@en .

eu-aiact:RecalledFromService a rdfs:Class,
        skos:Concept,
        eu-aiact:ServiceSupplyStatus ;
    dct:contributor _:person-delaram-golpayegani ;
    dct:created "2024-05-17"^^xsd:date ;
    rdfs:isDefinedBy eu-aiact: ;
    sw:term_status "accepted"@en ;
    skos:broader eu-aiact:ServiceSupplyStatus ;
    skos:definition "An AI system that is returned to the provider or taken out of service or use"@en ;
    skos:inScheme eu-aiact:status-classes ;
    skos:prefLabel "Recalled from Service"@en .

eu-aiact:RemoteBiometricIdentificationSystem a rdfs:Class,
        skos:Concept,
        eu-aiact:AISystem ;
    dct:contributor _:person-delaram-golpayegani ;
    dct:created "2024-04-10"^^xsd:date ;
    dct:modified "2025-07-30"^^xsd:date ;
    dct:source "AIA(Art. 3(41))"@en ;
    rdfs:isDefinedBy eu-aiact: ;
    sw:term_status "modified"@en ;
    skos:broader eu-aiact:AISystem ;
    skos:definition "An AI system for the purpose of identifying natural persons, without their active involvement, typically at a distance through the comparison of a person’s biometric data with the biometric data contained in a reference database."@en ;
    skos:inScheme eu-aiact:system-classes ;
    skos:prefLabel "Remote Biometric Identification System"@en ;
    skos:related pd:Biometric .

eu-aiact:Risk a rdfs:Class,
        skos:Concept ;
    dct:contributor _:person-delaram-golpayegani ;
    dct:created "2024-04-10"^^xsd:date ;
    dct:modified "2025-07-30"^^xsd:date ;
    dct:source "AIA (Art. 3(2))"@en ;
    rdfs:isDefinedBy eu-aiact: ;
    rdfs:subClassOf dpv:Risk ;
    sw:term_status "modified"@en ;
    skos:broader dpv:Risk ;
    skos:definition "The combination of the probability of an occurrence of harm and the severity of that harm"@en ;
    skos:inScheme eu-aiact:risk-classes ;
    skos:prefLabel "Risk"@en .

eu-aiact:RiskLevel a rdfs:Class,
        skos:Concept ;
    dct:contributor _:person-arthit-suriyawongkul,
        _:person-delaram-golpayegani,
        _:person-georg-p-krog,
        _:person-harshvardhan-j-pandit ;
    dct:created "2025-04-03"^^xsd:date ;
    dct:source "AI Act"@en ;
    rdfs:isDefinedBy eu-aiact: ;
    rdfs:subClassOf dpv:RiskLevel ;
    sw:term_status "accepted"@en ;
    skos:broader dpv:RiskLevel ;
    skos:definition "Enumeration of AI Act's risk-based categorisation which determines the prohibitions and obligations for AI systems"@en ;
    skos:inScheme eu-aiact:risk-levels-classes ;
    skos:prefLabel "Risk Level"@en .

eu-aiact:RiskLevelHigh a rdfs:Class,
        skos:Concept,
        eu-aiact:RiskLevel ;
    dct:contributor _:person-arthit-suriyawongkul,
        _:person-delaram-golpayegani,
        _:person-georg-p-krog,
        _:person-harshvardhan-j-pandit ;
    dct:created "2025-04-03"^^xsd:date ;
    dct:source "AIA(Art.6)"@en ;
    rdfs:isDefinedBy eu-aiact: ;
    sw:term_status "accepted"@en ;
    skos:broader eu-aiact:RiskLevelPermitted ;
    skos:definition "Risk Level categorising an AI system as \"high-risk\" as defined in the AI Act"@en ;
    skos:inScheme eu-aiact:risk-levels-classes ;
    skos:prefLabel "Risk Level - High"@en .

eu-aiact:RiskLevelHighAnnexI a rdfs:Class,
        skos:Concept,
        eu-aiact:RiskLevel ;
    dct:contributor _:person-arthit-suriyawongkul,
        _:person-delaram-golpayegani,
        _:person-georg-p-krog,
        _:person-harshvardhan-j-pandit ;
    dct:created "2025-04-03"^^xsd:date ;
    dct:source "AIA(Anx.I)"@en ;
    rdfs:isDefinedBy eu-aiact: ;
    sw:term_status "accepted"@en ;
    skos:broader eu-aiact:RiskLevelHigh ;
    skos:definition "Risk Level categorising an AI system as \"high-risk\" as defined in the AI Act Annex I"@en ;
    skos:inScheme eu-aiact:risk-levels-classes ;
    skos:prefLabel "Risk Level - High per Annex I"@en .

eu-aiact:RiskLevelHighAnnexIII a rdfs:Class,
        skos:Concept,
        eu-aiact:RiskLevel ;
    dct:contributor _:person-arthit-suriyawongkul,
        _:person-delaram-golpayegani,
        _:person-georg-p-krog,
        _:person-harshvardhan-j-pandit ;
    dct:created "2025-04-03"^^xsd:date ;
    dct:source "AIA(Anx.III)"@en ;
    rdfs:isDefinedBy eu-aiact: ;
    sw:term_status "accepted"@en ;
    skos:broader eu-aiact:RiskLevelHigh ;
    skos:definition "Risk Level categorising an AI system as \"high-risk\" as defined in the AI Act Annex III"@en ;
    skos:inScheme eu-aiact:risk-levels-classes ;
    skos:prefLabel "Risk Level - High per Annex III"@en .

eu-aiact:RiskLevelMinimal a rdfs:Class,
        skos:Concept,
        eu-aiact:RiskLevel ;
    dct:contributor _:person-arthit-suriyawongkul,
        _:person-delaram-golpayegani,
        _:person-georg-p-krog,
        _:person-harshvardhan-j-pandit ;
    dct:created "2025-04-03"^^xsd:date ;
    rdfs:isDefinedBy eu-aiact: ;
    sw:term_status "accepted"@en ;
    skos:broader eu-aiact:RiskLevelNotHigh ;
    skos:definition "Risk Level categorising an AI system as not being prohibited or high-risk or transparency required as defined in the AI Act"@en ;
    skos:inScheme eu-aiact:risk-levels-classes ;
    skos:prefLabel "Risk Level - Minimal"@en ;
    skos:scopeNote "The minimal risk level does not indicate there is no risk, but instead indicates that it is not sufficient to be regulated under the categorisations of the AI Act"@en .

eu-aiact:RiskLevelNotHigh a rdfs:Class,
        skos:Concept,
        eu-aiact:RiskLevel ;
    dct:contributor _:person-arthit-suriyawongkul,
        _:person-delaram-golpayegani,
        _:person-georg-p-krog,
        _:person-harshvardhan-j-pandit ;
    dct:created "2025-04-03"^^xsd:date ;
    rdfs:isDefinedBy eu-aiact: ;
    sw:term_status "accepted"@en ;
    skos:broader eu-aiact:RiskLevelPermitted ;
    skos:definition "Risk Level categorising an AI system as not being \"high-risk\" as defined in the AI Act"@en ;
    skos:inScheme eu-aiact:risk-levels-classes ;
    skos:prefLabel "Risk Level - Not High"@en ;
    skos:scopeNote "The \"not high\" risk level is useful for indicating the outcomes of assessments determining whether something is high-risk"@en .

eu-aiact:RiskLevelPermitted a rdfs:Class,
        skos:Concept,
        eu-aiact:RiskLevel ;
    dct:contributor _:person-arthit-suriyawongkul,
        _:person-delaram-golpayegani,
        _:person-georg-p-krog,
        _:person-harshvardhan-j-pandit ;
    dct:created "2025-04-03"^^xsd:date ;
    rdfs:isDefinedBy eu-aiact: ;
    sw:term_status "accepted"@en ;
    skos:broader eu-aiact:RiskLevel ;
    skos:definition "Concept representing \"AI practices\" are permitted i.e. not prohibited under the AI Act"@en ;
    skos:inScheme eu-aiact:risk-levels-classes ;
    skos:prefLabel "Risk Level - Permitted"@en ;
    skos:scopeNote "The permitted risk level is useful for representing outcomes of assessments determining whether something is prohibited"@en .

eu-aiact:RiskLevelProhibited a rdfs:Class,
        skos:Concept,
        eu-aiact:RiskLevel ;
    dct:contributor _:person-arthit-suriyawongkul,
        _:person-delaram-golpayegani,
        _:person-georg-p-krog,
        _:person-harshvardhan-j-pandit ;
    dct:created "2025-04-03"^^xsd:date ;
    dct:source "AIA(Art.5)"@en ;
    rdfs:isDefinedBy eu-aiact: ;
    sw:term_status "accepted"@en ;
    skos:broader eu-aiact:RiskLevel ;
    skos:definition "Risk Level prohibiting \"AI practices\" as defined in the AI Act"@en ;
    skos:inScheme eu-aiact:risk-levels-classes ;
    skos:prefLabel "Risk Level - Prohibited"@en .

eu-aiact:RiskLevelTransparencyRequired a rdfs:Class,
        skos:Concept,
        eu-aiact:RiskLevel ;
    dct:contributor _:person-arthit-suriyawongkul,
        _:person-delaram-golpayegani,
        _:person-georg-p-krog,
        _:person-harshvardhan-j-pandit ;
    dct:created "2025-04-03"^^xsd:date ;
    dct:source "AIA(Art.50)"@en ;
    rdfs:isDefinedBy eu-aiact: ;
    sw:term_status "accepted"@en ;
    skos:broader eu-aiact:RiskLevelNotHigh ;
    skos:definition "Risk Level categorising an AI system as not high-risk but where transparency is require as defined in the AI Act"@en ;
    skos:inScheme eu-aiact:risk-levels-classes ;
    skos:prefLabel "Risk Level - Transparency Required"@en .

eu-aiact:RiskManagementSystem a rdfs:Class,
        skos:Concept ;
    dct:contributor _:person-delaram-golpayegani ;
    dct:created "2024-06-12"^^xsd:date ;
    dct:source "AI Act"@en ;
    rdfs:isDefinedBy eu-aiact: ;
    rdfs:subClassOf risk:RiskManagement ;
    sw:term_status "accepted"@en ;
    skos:broader risk:RiskManagement ;
    skos:definition "A risk management system is a continuous iterative process planned and run throughout the entire lifecycle of a high-risk AI system, requiring regular systematic review and updating"@en ;
    skos:inScheme eu-aiact:risk-classes ;
    skos:prefLabel "Risk Management System"@en .

eu-aiact:SafetyComponent a rdfs:Class,
        skos:Concept ;
    dct:contributor _:person-delaram-golpayegani ;
    dct:created "2024-04-10"^^xsd:date ;
    dct:modified "2025-07-30"^^xsd:date ;
    dct:source "AIA (Art. 3(14))"@en ;
    rdfs:isDefinedBy eu-aiact: ;
    rdfs:subClassOf tech:Component ;
    sw:term_status "modified"@en ;
    skos:broader tech:Component ;
    skos:definition "A component of a product or of an AI system which fulfils a safety function for that product or AI system, or the failure or malfunctioning of which endangers the health and safety of persons or property"@en ;
    skos:inScheme eu-aiact:system-classes ;
    skos:prefLabel "Safety Component"@en .

eu-aiact:SandboxPlan a rdfs:Class,
        skos:Concept,
        tech:Documentation ;
    dct:contributor _:person-delaram-golpayegani ;
    dct:created "2024-04-10"^^xsd:date ;
    dct:modified "2025-07-31"^^xsd:date ;
    dct:source "AIA (Art.3(54))"@en ;
    rdfs:isDefinedBy eu-aiact: ;
    sw:term_status "modified"@en ;
    skos:broader tech:Plan ;
    skos:definition "A document agreed between the participating provider and the competent authority describing the objectives, conditions, timeframe, methodology and requirements for the activities carried out within the sandbox"@en ;
    skos:inScheme eu-aiact:docs-classes ;
    skos:prefLabel "Sandbox Plan"@en .

eu-aiact:SeriousIncident a rdfs:Class,
        skos:Concept ;
    dct:contributor _:person-delaram-golpayegani ;
    dct:created "2024-04-10"^^xsd:date ;
    dct:modified "2025-07-30"^^xsd:date ;
    dct:source "AIA (Art. 3(49))"@en ;
    rdfs:isDefinedBy eu-aiact: ;
    rdfs:subClassOf risk:Incident ;
    sw:term_status "modified"@en ;
    skos:broader risk:Incident ;
    skos:definition """an incident or malfunctioning of an AI system that directly or indirectly leads to any of the following:
(a) the death of a person, or serious harm to a person’s health;
(b) a serious and irreversible disruption of the management or operation of critical infrastructure;
(c) the infringement of obligations under Union law intended to protect fundamental rights;
(d) serious harm to property or the environment;"""@en ;
    skos:inScheme eu-aiact:risk-classes ;
    skos:prefLabel "Serious Incident"@en .

eu-aiact:ServiceSupplyStatus a rdfs:Class,
        skos:Concept ;
    dct:contributor _:person-delaram-golpayegani ;
    dct:created "2024-05-17"^^xsd:date ;
    rdfs:isDefinedBy eu-aiact: ;
    rdfs:subClassOf tech:ProvisionStatus ;
    sw:term_status "accepted"@en ;
    skos:broader tech:ProvisionStatus ;
    skos:definition "Status associated with whether the AI system has been supplied for use or put in to service or been recalled or withdrawn"@en ;
    skos:inScheme eu-aiact:status-classes ;
    skos:prefLabel "Service Supply Status"@en .

eu-aiact:SubstantialModification a rdfs:Class,
        skos:Concept ;
    dct:contributor _:person-delaram-golpayegani ;
    dct:created "2024-04-10"^^xsd:date ;
    dct:modified "2025-07-30"^^xsd:date ;
    dct:source "AIA(Art. 3(23))"@en ;
    rdfs:isDefinedBy eu-aiact: ;
    sw:term_status "modified"@en ;
    skos:definition "A change to an AI system after its placing on the market or putting into service which is not foreseen or planned in the initial conformity assessment carried out by the provider and as a result of which the compliance of the AI system with the requirements set out in Chapter III, Section 2 is affected or results in a modification to the intended purpose for which the AI system has been assessed"@en ;
    skos:inScheme eu-aiact:misc-classes ;
    skos:prefLabel "Substantial Modification"@en .

eu-aiact:SystemArchitectureDescription a rdfs:Class,
        skos:Concept,
        tech:Documentation ;
    dct:contributor _:person-delaram-golpayegani ;
    dct:created "2024-12-01"^^xsd:date ;
    dct:source "AI Act Annex.IV"@en ;
    rdfs:isDefinedBy eu-aiact: ;
    sw:term_status "accepted"@en ;
    skos:broader tech:Documentation ;
    skos:definition "Documentation specifying the software architecture"@en ;
    skos:inScheme eu-aiact:docs-classes ;
    skos:prefLabel "System Architecture Description"@en .

eu-aiact:SystemicRisk a rdfs:Class,
        skos:Concept ;
    dct:contributor _:person-delaram-golpayegani ;
    dct:created "2024-04-10"^^xsd:date ;
    dct:modified "2025-07-30"^^xsd:date ;
    dct:source "AIA(Art.3 (65))"@en ;
    rdfs:isDefinedBy eu-aiact: ;
    rdfs:subClassOf eu-aiact:Risk ;
    sw:term_status "modified"@en ;
    skos:broader eu-aiact:Risk ;
    skos:definition "Q risk that is specific to the high-impact capabilities of general-purpose AI models, having a significant impact on the Union market due to their reach, or due to actual or reasonably foreseeable negative effects on public health, safety, public security, fundamental rights, or the society as a whole, that can be propagated at scale across the value chain"@en ;
    skos:inScheme eu-aiact:risk-classes ;
    skos:prefLabel "Systemic Risk"@en .

eu-aiact:TechnicalDocumentation a rdfs:Class,
        skos:Concept,
        tech:Documentation ;
    dct:contributor _:person-delaram-golpayegani ;
    dct:created "2024-04-10"^^xsd:date ;
    dct:modified "2024-12-17"^^xsd:date ;
    dct:source " AIA Annex.IV"@en,
        "AIA Art.11"@en ;
    rdfs:isDefinedBy eu-aiact: ;
    sw:term_status "modified"@en ;
    skos:broader tech:Documentation ;
    skos:definition "Annex IV technical documentation"@en ;
    skos:inScheme eu-aiact:docs-classes ;
    skos:prefLabel "Technical Documentation"@en .

eu-aiact:TestLog a rdfs:Class,
        skos:Concept,
        tech:Documentation ;
    dct:contributor _:person-delaram-golpayegani ;
    dct:created "2024-12-01"^^xsd:date ;
    dct:source "AI Act Annex.IV"@en ;
    rdfs:isDefinedBy eu-aiact: ;
    sw:term_status "accepted"@en ;
    skos:broader tech:Documentation ;
    skos:definition "Log of the tests performed"@en ;
    skos:inScheme eu-aiact:docs-classes ;
    skos:prefLabel "Test Log"@en .

eu-aiact:TestReport a rdfs:Class,
        skos:Concept,
        tech:Documentation ;
    dct:contributor _:person-delaram-golpayegani ;
    dct:created "2024-12-01"^^xsd:date ;
    dct:source "AI Act Annex.IV"@en ;
    rdfs:isDefinedBy eu-aiact: ;
    sw:term_status "accepted"@en ;
    skos:broader tech:Documentation ;
    skos:definition "A document that includes a summary of test activities and their results"@en ;
    skos:inScheme eu-aiact:docs-classes ;
    skos:prefLabel "Test Report"@en .

eu-aiact:TestingData a rdfs:Class,
        skos:Concept ;
    dct:contributor _:person-delaram-golpayegani ;
    dct:created "2024-04-10"^^xsd:date ;
    dct:modified "2025-07-30"^^xsd:date ;
    dct:source "AIA (Art. 3(32))"@en ;
    rdfs:isDefinedBy eu-aiact: ;
    rdfs:subClassOf ai:TestingData ;
    sw:term_status "modified"@en ;
    skos:broader ai:TestingData ;
    skos:definition "Data used for providing an independent evaluation of the AI system in order to confirm the expected performance of that system before its placing on the market or putting into service"@en ;
    skos:inScheme eu-aiact:data-classes ;
    skos:prefLabel "Testing Data"@en .

eu-aiact:TestingRealWorldConditions a rdfs:Class,
        skos:Concept,
        dpv:OrganisationalMeasure ;
    dct:contributor _:person-delaram-golpayegani ;
    dct:created "2024-04-10"^^xsd:date ;
    dct:modified "2024-07-30"^^xsd:date ;
    dct:source "AIA (Art. 3(57))"@en ;
    rdfs:isDefinedBy eu-aiact: ;
    sw:term_status "modified"@en ;
    skos:broader dpv:OrganisationalMeasure ;
    skos:definition "The temporary testing of an AI system for its intended purpose in real-world conditions outside a laboratory or otherwise simulated environment, with a view to gathering reliable and robust data and to assessing and verifying the conformity of the AI system with the requirements of the AI Act and it does not qualify as placing the AI system on the market or putting it into service within the meaning of the AI Act, provided that all the conditions laid down in Article 57 or 60 are fulfilled"@en ;
    skos:inScheme eu-aiact:assessment-classes ;
    skos:prefLabel "Testing In Real World Conditions"@en .

eu-aiact:TrainingData a rdfs:Class,
        skos:Concept ;
    dct:contributor _:person-delaram-golpayegani ;
    dct:created "2024-04-10"^^xsd:date ;
    dct:modified "2024-12-01"^^xsd:date ;
    dct:source "AIA(Art. 3(29))"@en ;
    rdfs:isDefinedBy eu-aiact: ;
    rdfs:subClassOf ai:TrainingData ;
    sw:term_status "modified"@en ;
    skos:broader ai:TrainingData ;
    skos:definition "Data used for training an AI system through fitting its learnable parameters"@en ;
    skos:inScheme eu-aiact:data-classes ;
    skos:prefLabel "Training Data"@en .

eu-aiact:ValidationData a rdfs:Class,
        skos:Concept ;
    dct:contributor _:person-delaram-golpayegani ;
    dct:created "2024-04-10"^^xsd:date ;
    dct:modified "2025-07-30"^^xsd:date ;
    dct:source "AIA (Art. 3(30))"@en ;
    rdfs:isDefinedBy eu-aiact: ;
    rdfs:subClassOf ai:ValidationData ;
    sw:term_status "modified"@en ;
    skos:broader ai:ValidationData ;
    skos:definition "Data used for providing an evaluation of the trained AI system and for tuning its non-learnable parameters and its learning process in order, inter alia, to prevent underfitting or overfitting"@en ;
    skos:inScheme eu-aiact:data-classes ;
    skos:prefLabel "Validation Data"@en .

eu-aiact:WithdrawnFromService a rdfs:Class,
        skos:Concept,
        eu-aiact:ServiceSupplyStatus ;
    dct:contributor _:person-delaram-golpayegani ;
    dct:created "2024-05-17"^^xsd:date ;
    rdfs:isDefinedBy eu-aiact: ;
    sw:term_status "accepted"@en ;
    skos:broader eu-aiact:ServiceSupplyStatus ;
    skos:definition "An AI system that is prevented to be made available in the supply chain"@en ;
    skos:inScheme eu-aiact:status-classes ;
    skos:prefLabel "Withdrawn from Service"@en .

<https://w3id.org/dpv/legal/eu/aiact> a owl:Ontology,
        profile:Profile ;
    dct:bibliographicCitation "Harshvardhan J. Pandit, Beatriz Esteves, Georg P. Krog, Paul Ryan, Delaram Golpayegani, Julian Flake (2025) Data Privacy Vocabulary (DPV) – Version 2.0. In: Demartini, G., et al. The Semantic Web – ISWC 2024. ISWC 2024. Lecture Notes in Computer Science, vol 15233. Springer, Cham. https://doi.org/10.1007/978-3-031-77847-6_10" ;
    dct:conformsTo "http://www.w3.org/2000/01/rdf-schema",
        "http://www.w3.org/2004/02/skos/core" ;
    dct:contributor _:person-arthit-suriyawongkul,
        _:person-beatriz-esteves,
        _:person-delaram-golpayegani,
        _:person-georg-p-krog,
        _:person-harshvardhan-j-pandit ;
    dct:created "2024-04-10"@en ;
    dct:creator _:person-delaram-golpayegani ;
    dct:description "Extension to the Data Privacy Vocabulary (DPV) providing concepts for representing information associated with EU AI Act"@en ;
    dct:identifier "https://w3id.org/dpv/legal/eu/aiact" ;
    dct:issued "2024-04-10"@en ;
    dct:license <https://www.w3.org/copyright/document-license-2023/> ;
    dct:modified "2025-08-01"@en ;
    dct:publisher <https://www.w3.org/> ;
    dct:source <https://www.w3.org/groups/cg/dpvcg/> ;
    dct:title "EU Artificial Intelligence Act (AI Act)"@en ;
    bibo:doi "10.5281/zenodo.12505841" ;
    bibo:status "http://purl.org/ontology/bibo/status/published" ;
    vann:preferredNamespacePrefix "eu-aiact" ;
    vann:preferredNamespaceUri "https://w3id.org/dpv/legal/eu/aiact#" ;
    rdfs:Label "EU-AIACT"@en ;
    owl:versionIRI <https://w3id.org/dpv/2.2/legal/eu/aiact> ;
    owl:versionInfo "2.2" ;
    profile:hasResource <https://w3id.org/dpv/examples>,
        <https://w3id.org/dpv/guides>,
        eu-aiact:serialisation-html,
        eu-aiact:serialisation-ttl,
        <https://w3id.org/dpv/primer> ;
    profile:isProfileOf rdfs:,
        skos:,
        <https://w3id.org/dpv> ;
    foaf:logo <https://w3id.org/dpv/media/logo.png> ;
    schema:version "2.2" .

eu-aiact:hasChangeCategory a rdf:Property,
        skos:Concept ;
    dcam:domainIncludes tech:AI ;
    dcam:rangeIncludes eu-aiact:ChangeCategory ;
    dct:contributor _:person-delaram-golpayegani ;
    dct:created "2024-12-01"^^xsd:date ;
    rdfs:isDefinedBy eu-aiact: ;
    rdfs:subPropertyOf dpv:hasContext ;
    sw:term_status "accepted"@en ;
    skos:broader dpv:hasContext ;
    skos:definition "Associates the category of change to the AI"@en ;
    skos:inScheme eu-aiact:status-properties ;
    skos:prefLabel "has change category"@en ;
    schema:domainIncludes tech:AI ;
    schema:rangeIncludes eu-aiact:ChangeCategory .

eu-aiact:hasChangeDescription a rdf:Property,
        skos:Concept ;
    dcam:domainIncludes tech:AI ;
    dcam:rangeIncludes eu-aiact:ChangeDescription ;
    dct:contributor _:person-delaram-golpayegani ;
    dct:created "2024-12-01"^^xsd:date ;
    rdfs:isDefinedBy eu-aiact: ;
    rdfs:subPropertyOf dpv:hasContext ;
    sw:term_status "accepted"@en ;
    skos:broader dpv:hasContext ;
    skos:definition "Associates the change description to AI"@en ;
    skos:inScheme eu-aiact:status-properties ;
    skos:prefLabel "has change description"@en ;
    schema:domainIncludes tech:AI ;
    schema:rangeIncludes eu-aiact:ChangeDescription .

eu-aiact:serialisation-html a profile:ResourceDescriptor ;
    dct:conformsTo <https://www.w3.org/TR/html/> ;
    dct:format <https://www.iana.org/assignments/media-types/text/html> ;
    dct:title "EU Artificial Intelligence Act (AI Act) - HTML serialisation" ;
    profile:hasArtifact <https://w3id.org/dpv/legal/eu/aiact/eu-aiact.html> ;
    profile:hasRole role:specification .

eu-aiact:serialisation-ttl a profile:ResourceDescriptor ;
    dct:conformsTo <https://www.w3.org/TR/turtle/> ;
    dct:format <https://www.iana.org/assignments/media-types/text/turtle> ;
    dct:title "EU Artificial Intelligence Act (AI Act) - Turtle serialisation" ;
    profile:hasArtifact <https://w3id.org/dpv/legal/eu/aiact/eu-aiact.ttl> ;
    profile:hasRole role:vocabulary .

<https://w3id.org/dpv/examples> a profile:ResourceDescriptor ;
    dct:conformsTo <https://www.w3.org/TR/html/> ;
    dct:format <https://www.iana.org/assignments/media-types/text/html> ;
    dct:title "Examples" ;
    profile:hasArtifact <https://w3id.org/dpv/examples> ;
    profile:hasRole role:guidance .

<https://w3id.org/dpv/guides> a profile:ResourceDescriptor ;
    dct:conformsTo <https://www.w3.org/TR/html/> ;
    dct:format <https://www.iana.org/assignments/media-types/text/html> ;
    dct:title "Guides for Data Privacy Vocabulary" ;
    profile:hasArtifact <https://w3id.org/dpv/guides> ;
    profile:hasRole role:guidance .

eu-aiact:status-properties a skos:ConceptScheme .

<https://w3id.org/dpv/primer> a profile:ResourceDescriptor ;
    dct:conformsTo <https://www.w3.org/TR/html/> ;
    dct:format <https://www.iana.org/assignments/media-types/text/html> ;
    dct:title "Primer for Data Privacy Vocabulary" ;
    profile:hasArtifact <https://w3id.org/dpv/primer> ;
    profile:hasRole role:guidance .

eu-aiact:compliance-classes a skos:ConceptScheme .

eu-aiact:data-classes a skos:ConceptScheme .

eu-aiact:risk-classes a skos:ConceptScheme .

eu-aiact:misc-classes a skos:ConceptScheme .

eu-aiact:capability-classes a skos:ConceptScheme .

eu-aiact:risk-levels-classes a skos:ConceptScheme .

eu-aiact:system-classes a skos:ConceptScheme .

eu-aiact:assessment-classes a skos:ConceptScheme .

eu-aiact:docs-classes a skos:ConceptScheme .

eu-aiact:sector-classes a skos:ConceptScheme .

eu-aiact:roles-classes a skos:ConceptScheme .

eu-aiact:status-classes a skos:ConceptScheme .

_:org-ai-accountability-lab-aial-trinity-college-dublin a foaf:Organization ;
    foaf:name "AI Accountability Lab (AIAL), Trinity College Dublin" .

_:org-idlab-imec-ghent-university a foaf:Organization ;
    foaf:name "IDLab, IMEC, Ghent University" .

_:org-signatu-as a foaf:Organization ;
    foaf:name "Signatu AS" .

_:org-adapt-centre-trinity-college-dublin a foaf:Organization ;
    foaf:name "ADAPT Centre, Trinity College Dublin" .

_:person-beatriz-esteves a dct:Agent,
        foaf:Person ;
    scoro:hasORCID "0000-0003-0259-7560" ;
    org:memberOf _:org-idlab-imec-ghent-university ;
    foaf:name "Beatriz Esteves" .

_:person-arthit-suriyawongkul a dct:Agent,
        foaf:Person ;
    scoro:hasORCID "0000-0002-9698-1899" ;
    org:memberOf _:org-adapt-centre-trinity-college-dublin ;
    foaf:name "Arthit Suriyawongkul" .

_:person-georg-p-krog a dct:Agent,
        foaf:Person ;
    org:memberOf _:org-signatu-as ;
    foaf:homepage "https://www.linkedin.com/in/georg-philip-krog-a2a278104/" ;
    foaf:name "Georg P. Krog" .

_:person-harshvardhan-j-pandit a dct:Agent,
        foaf:Person ;
    scoro:hasORCID "0000-0002-5068-3714" ;
    org:memberOf _:org-ai-accountability-lab-aial-trinity-college-dublin ;
    foaf:homepage "https://harshp.com/" ;
    foaf:name "Harshvardhan J. Pandit" .

_:person-delaram-golpayegani a dct:Agent,
        foaf:Person ;
    scoro:hasORCID "0000-0002-1208-186X" ;
    org:memberOf _:org-adapt-centre-trinity-college-dublin ;
    foaf:name "Delaram Golpayegani" .

