@prefix bibo: <http://purl.org/ontology/bibo/> .
@prefix dct: <http://purl.org/dc/terms/> .
@prefix dpv: <https://w3id.org/dpv#> .
@prefix eu-nis2: <https://w3id.org/dpv/legal/eu/nis2#> .
@prefix foaf: <http://xmlns.com/foaf/0.1/> .
@prefix org: <http://www.w3.org/ns/org#> .
@prefix owl: <http://www.w3.org/2002/07/owl#> .
@prefix profile: <http://www.w3.org/ns/dx/prof/> .
@prefix rdf: <http://www.w3.org/1999/02/22-rdf-syntax-ns#> .
@prefix rdfs: <http://www.w3.org/2000/01/rdf-schema#> .
@prefix risk: <https://w3id.org/dpv/risk#> .
@prefix role: <http://www.w3.org/ns/dx/prof/role/> .
@prefix schema: <https://schema.org/> .
@prefix scoro: <http://purl.org/spar/scoro/> .
@prefix skos: <http://www.w3.org/2004/02/skos/core#> .
@prefix sw: <http://www.w3.org/2003/06/sw-vocab-status/ns#> .
@prefix vann: <http://purl.org/vocab/vann/> .
@prefix xsd: <http://www.w3.org/2001/XMLSchema#> .

eu-nis2:EarlyWarningReport a rdfs:Class,
        skos:Concept,
        risk:IncidentNotice ;
    dct:contributor _:N05cd1f43dbaf4b4ba297dab5ee221394,
        _:N0a43dd9ea5e94fe695d8b7df8802cfdd ;
    dct:created "2024-05-19"^^xsd:date ;
    dct:source "NIS2 Directive"@en ;
    rdfs:isDefinedBy eu-nis2: ;
    sw:term_status "accepted"@en ;
    skos:broader risk:IncidentNotice ;
    skos:definition "within 24 hours of detection containing cause of the  incident and whether it was unlawful or malicious and whether there is  cross-border impact"@en ;
    skos:inScheme eu-nis2:notice-classes ;
    skos:prefLabel "Early Warning Report"@en .

eu-nis2:FinalReport a rdfs:Class,
        skos:Concept,
        risk:IncidentNotice ;
    dct:contributor _:N05cd1f43dbaf4b4ba297dab5ee221394,
        _:N0a43dd9ea5e94fe695d8b7df8802cfdd ;
    dct:created "2024-05-19"^^xsd:date ;
    dct:source "NIS2 Directive"@en ;
    rdfs:isDefinedBy eu-nis2: ;
    sw:term_status "accepted"@en ;
    skos:broader risk:IncidentNotice ;
    skos:definition "within 1 month of incident handling i.e.  completing the incident recovery and containing the  applied/ongoing measures, 'detailed description' - not sure what this  means, and threat type / root cause - which is covered with threat and  vulnerability concepts"@en ;
    skos:inScheme eu-nis2:notice-classes ;
    skos:prefLabel "Final Report"@en .

eu-nis2:IncidentAssessmentReport a rdfs:Class,
        skos:Concept,
        risk:IncidentNotice ;
    dct:contributor _:N05cd1f43dbaf4b4ba297dab5ee221394,
        _:N0a43dd9ea5e94fe695d8b7df8802cfdd ;
    dct:created "2024-05-19"^^xsd:date ;
    dct:source "NIS2 Directive"@en ;
    rdfs:isDefinedBy eu-nis2: ;
    sw:term_status "accepted"@en ;
    skos:broader risk:IncidentNotice ;
    skos:definition "within 72 hours of detection, which contains  updates on the earlier information as well as initial assessment of  severity and impact of the incident as well as any 'indicators of  compromise'"@en ;
    skos:inScheme eu-nis2:notice-classes ;
    skos:prefLabel "Incident Assessment Report"@en .

eu-nis2:InitialFeedbackOnIncident a rdfs:Class,
        skos:Concept,
        risk:IncidentNotice ;
    dct:contributor _:N05cd1f43dbaf4b4ba297dab5ee221394,
        _:N0a43dd9ea5e94fe695d8b7df8802cfdd ;
    dct:created "2024-05-19"^^xsd:date ;
    dct:source "NIS2 Directive"@en ;
    rdfs:isDefinedBy eu-nis2: ;
    sw:term_status "accepted"@en ;
    skos:broader risk:IncidentNotice ;
    skos:definition "Notification from authority to organisation (upon request, within 24 hours or early warning) containing  \"initial feedback\" and guidelines on measures that can be taken in  response to a breach"@en ;
    skos:inScheme eu-nis2:notice-classes ;
    skos:prefLabel "Initial Feedback on Incident"@en .

eu-nis2:IntermediateReport a rdfs:Class,
        skos:Concept,
        risk:IncidentNotice ;
    dct:contributor _:N05cd1f43dbaf4b4ba297dab5ee221394,
        _:N0a43dd9ea5e94fe695d8b7df8802cfdd ;
    dct:created "2024-05-19"^^xsd:date ;
    dct:source "NIS2 Directive"@en ;
    rdfs:isDefinedBy eu-nis2: ;
    sw:term_status "accepted"@en ;
    skos:broader risk:IncidentNotice ;
    skos:definition "upon request - which provides updates, if any,  to previous information"@en ;
    skos:inScheme eu-nis2:notice-classes ;
    skos:prefLabel "Intermediate Report"@en .

eu-nis2:NIS2ComplianceUnknown a rdfs:Class,
        skos:Concept,
        dpv:Lawfulness ;
    dct:contributor _:N0a43dd9ea5e94fe695d8b7df8802cfdd,
        _:N458008bc6195484e9cc557f70eabda31 ;
    dct:created "2024-07-21"^^xsd:date ;
    rdfs:isDefinedBy eu-nis2: ;
    sw:term_status "accepted"@en ;
    skos:broader eu-nis2:NIS2Lawfulness ;
    skos:definition "State where lawfulness or compliance with NIS2 is unknown"@en ;
    skos:inScheme eu-nis2:compliance-classes ;
    skos:prefLabel "NIS2 Compliance Unknown"@en .

eu-nis2:NIS2Compliant a rdfs:Class,
        skos:Concept,
        dpv:Lawfulness ;
    dct:contributor _:N0a43dd9ea5e94fe695d8b7df8802cfdd,
        _:N458008bc6195484e9cc557f70eabda31 ;
    dct:created "2024-07-21"^^xsd:date ;
    rdfs:isDefinedBy eu-nis2: ;
    sw:term_status "accepted"@en ;
    skos:broader eu-nis2:NIS2Lawfulness ;
    skos:definition "State of being lawful or legally compliant for NIS2"@en ;
    skos:inScheme eu-nis2:compliance-classes ;
    skos:prefLabel "NIS2 Compliant"@en .

eu-nis2:NIS2Lawfulness a rdfs:Class,
        skos:Concept,
        dpv:Lawfulness ;
    dct:contributor _:N0a43dd9ea5e94fe695d8b7df8802cfdd,
        _:N458008bc6195484e9cc557f70eabda31 ;
    dct:created "2024-07-21"^^xsd:date ;
    rdfs:isDefinedBy eu-nis2: ;
    sw:term_status "accepted"@en ;
    skos:broader dpv:Lawfulness ;
    skos:definition "Status or state associated with being lawful or legally compliant regarding NIS2"@en ;
    skos:inScheme eu-nis2:compliance-classes ;
    skos:prefLabel "NIS2 Lawfulness"@en .

eu-nis2:NIS2NonCompliant a rdfs:Class,
        skos:Concept,
        dpv:Lawfulness ;
    dct:contributor _:N0a43dd9ea5e94fe695d8b7df8802cfdd,
        _:N458008bc6195484e9cc557f70eabda31 ;
    dct:created "2024-07-21"^^xsd:date ;
    rdfs:isDefinedBy eu-nis2: ;
    sw:term_status "accepted"@en ;
    skos:broader eu-nis2:NIS2Lawfulness ;
    skos:definition "State of being unlawful or legally non-compliant for NIS2"@en ;
    skos:inScheme eu-nis2:compliance-classes ;
    skos:prefLabel "NIS2 Non-compliant"@en .

eu-nis2:ProgressReport a rdfs:Class,
        skos:Concept,
        risk:IncidentNotice ;
    dct:contributor _:N05cd1f43dbaf4b4ba297dab5ee221394,
        _:N0a43dd9ea5e94fe695d8b7df8802cfdd ;
    dct:created "2024-05-19"^^xsd:date ;
    dct:source "NIS2 Directive"@en ;
    rdfs:isDefinedBy eu-nis2: ;
    sw:term_status "accepted"@en ;
    skos:broader risk:IncidentNotice ;
    skos:definition "within 1 month of detection if the  incident handling has not been completed by then, with updates to  previous information"@en ;
    skos:inScheme eu-nis2:notice-classes ;
    skos:prefLabel "Progress Report"@en .

eu-nis2:RiskMitigationAdvice a rdfs:Class,
        skos:Concept,
        risk:IncidentNotice ;
    dct:contributor _:N05cd1f43dbaf4b4ba297dab5ee221394,
        _:N0a43dd9ea5e94fe695d8b7df8802cfdd ;
    dct:created "2024-05-19"^^xsd:date ;
    dct:source "NIS2 Directive"@en ;
    rdfs:isDefinedBy eu-nis2: ;
    sw:term_status "accepted"@en ;
    skos:broader risk:IncidentNotice ;
    skos:definition "Notification from organisation to stakeholders regarding risk mitigations to be applied and existence of threats"@en ;
    skos:inScheme eu-nis2:notice-classes ;
    skos:prefLabel "Risk Mitigation Advice"@en .

eu-nis2:SignificantIncidentNotice a rdfs:Class,
        skos:Concept ;
    dct:contributor _:N05cd1f43dbaf4b4ba297dab5ee221394,
        _:N0a43dd9ea5e94fe695d8b7df8802cfdd ;
    dct:created "2024-05-19"^^xsd:date ;
    dct:source "NIS2 Directive"@en ;
    rdfs:isDefinedBy eu-nis2: ;
    rdfs:subClassOf risk:IncidentNotice ;
    sw:term_status "accepted"@en ;
    skos:broader risk:IncidentNotice ;
    skos:definition "Notice sent for reporting significant incidents"@en ;
    skos:inScheme eu-nis2:notice-classes ;
    skos:prefLabel "Significant Incident Notice"@en .

<https://w3id.org/dpv/legal/eu/nis2> a owl:Ontology,
        profile:Profile ;
    dct:bibliographicCitation "Harshvardhan J. Pandit, Beatriz Esteves, Georg P. Krog, Paul Ryan, Delaram Golpayegani, Julian Flake (2025) Data Privacy Vocabulary (DPV) – Version 2.0. In: Demartini, G., et al. The Semantic Web – ISWC 2024. ISWC 2024. Lecture Notes in Computer Science, vol 15233. Springer, Cham. https://doi.org/10.1007/978-3-031-77847-6_10" ;
    dct:conformsTo "http://www.w3.org/2000/01/rdf-schema",
        "http://www.w3.org/2004/02/skos/core" ;
    dct:contributor _:N05cd1f43dbaf4b4ba297dab5ee221394,
        _:N0a43dd9ea5e94fe695d8b7df8802cfdd,
        _:N458008bc6195484e9cc557f70eabda31 ;
    dct:created "2024-05-19"@en ;
    dct:creator _:N05cd1f43dbaf4b4ba297dab5ee221394,
        _:N0a43dd9ea5e94fe695d8b7df8802cfdd ;
    dct:description "Extension to the Data Privacy Vocabulary (DPV) providing concepts for representing  information associated with EU NIS2"@en ;
    dct:identifier "https://w3id.org/dpv/legal/eu/nis2" ;
    dct:issued "2024-05-19"@en ;
    dct:license <https://www.w3.org/copyright/document-license-2023/> ;
    dct:modified "2025-03-16"@en ;
    dct:publisher <https://www.w3.org/> ;
    dct:source <https://www.w3.org/groups/cg/dpvcg/> ;
    dct:title "EU Network and Information Services Directive (NIS2)"@en ;
    bibo:doi "10.5281/zenodo.12505841" ;
    bibo:status "http://purl.org/ontology/bibo/status/published" ;
    vann:preferredNamespacePrefix "eu-nis2" ;
    vann:preferredNamespaceUri "https://w3id.org/dpv/legal/eu/nis2#" ;
    rdfs:Label "EU-NIS2"@en ;
    owl:versionIRI <https://w3id.org/dpv/2.1/legal/eu/nis2> ;
    owl:versionInfo "2.1" ;
    profile:hasResource <https://w3id.org/dpv/examples>,
        <https://w3id.org/dpv/guides>,
        eu-nis2:serialisation-html,
        eu-nis2:serialisation-jsonld,
        eu-nis2:serialisation-n3,
        eu-nis2:serialisation-rdf,
        eu-nis2:serialisation-ttl,
        <https://w3id.org/dpv/primer> ;
    profile:isProfileOf rdfs:,
        skos:,
        <https://w3id.org/dpv> ;
    foaf:logo <https://w3id.org/dpv/media/logo.png> ;
    schema:version "2.1" .

eu-nis2:serialisation-html a profile:ResourceDescriptor ;
    dct:conformsTo <https://www.w3.org/TR/html/> ;
    dct:format <https://www.iana.org/assignments/media-types/text/html> ;
    dct:title "EU Network and Information Services Directive (NIS2) - HTML serialiation" ;
    profile:hasArtifact <https://w3id.org/dpv/legal/eu/nis2/eu-nis2.html> ;
    profile:hasRole role:specification .

eu-nis2:serialisation-jsonld a profile:ResourceDescriptor ;
    dct:conformsTo <https://www.w3.org/TR/json-ld11/> ;
    dct:format <https://www.iana.org/assignments/media-types/application/ld+json> ;
    dct:title "EU Network and Information Services Directive (NIS2) - JSON-LD serialiation" ;
    profile:hasArtifact <https://w3id.org/dpv/legal/eu/nis2/eu-nis2.jsonld> ;
    profile:hasRole role:vocabulary .

eu-nis2:serialisation-n3 a profile:ResourceDescriptor ;
    dct:conformsTo <https://www.w3.org/TeamSubmission/n3/> ;
    dct:format <https://www.iana.org/assignments/media-types/text/n3> ;
    dct:title "EU Network and Information Services Directive (NIS2) - N3 serialiation" ;
    profile:hasArtifact <https://w3id.org/dpv/legal/eu/nis2/eu-nis2.n3> ;
    profile:hasRole role:vocabulary .

eu-nis2:serialisation-rdf a profile:ResourceDescriptor ;
    dct:conformsTo rdf: ;
    dct:format <https://www.iana.org/assignments/media-types/application/rdf+xml> ;
    dct:title "EU Network and Information Services Directive (NIS2) - RDF/XML serialiation" ;
    profile:hasArtifact <https://w3id.org/dpv/legal/eu/nis2/eu-nis2.rdf> ;
    profile:hasRole role:vocabulary .

eu-nis2:serialisation-ttl a profile:ResourceDescriptor ;
    dct:conformsTo <https://www.w3.org/TR/turtle/> ;
    dct:format <https://www.iana.org/assignments/media-types/text/turtle> ;
    dct:title "EU Network and Information Services Directive (NIS2) - Turtle serialiation" ;
    profile:hasArtifact <https://w3id.org/dpv/legal/eu/nis2/eu-nis2.ttl> ;
    profile:hasRole role:vocabulary .

<https://w3id.org/dpv/examples> a profile:ResourceDescriptor ;
    dct:conformsTo <https://www.w3.org/TR/html/> ;
    dct:format <https://www.iana.org/assignments/media-types/text/html> ;
    dct:title "Examples for Data Privacy Vocabulary" ;
    profile:hasArtifact <https://w3id.org/dpv/examples> ;
    profile:hasRole role:guidance .

<https://w3id.org/dpv/guides> a profile:ResourceDescriptor ;
    dct:conformsTo <https://www.w3.org/TR/html/> ;
    dct:format <https://www.iana.org/assignments/media-types/text/html> ;
    dct:title "Guides for Data Privacy Vocabulary" ;
    profile:hasArtifact <https://w3id.org/dpv/guides> ;
    profile:hasRole role:guidance .

<https://w3id.org/dpv/primer> a profile:ResourceDescriptor ;
    dct:conformsTo <https://www.w3.org/TR/html/> ;
    dct:format <https://www.iana.org/assignments/media-types/text/html> ;
    dct:title "Primer for Data Privacy Vocabulary" ;
    profile:hasArtifact <https://w3id.org/dpv/primer> ;
    profile:hasRole role:guidance .

eu-nis2:compliance-classes a skos:ConceptScheme .

eu-nis2:notice-classes a skos:ConceptScheme .

_:N2bfb2dfcc0b24c5182bd06c242c085fa a foaf:Organization ;
    foaf:name "Signatu AS" .

_:N313d89a6c37147bfac1bbb4aa7f6510b a foaf:Organization ;
    foaf:name "ADAPT Centre, Dublin City University" .

_:N3f64d3533a104953b63bb217ff4665c5 a foaf:Organization ;
    foaf:name "IDLab, IMEC, Ghent University" .

_:N458008bc6195484e9cc557f70eabda31 a dct:Agent,
        foaf:Person ;
    scoro:hasORCID "0000-0003-0259-7560" ;
    org:memberOf _:N3f64d3533a104953b63bb217ff4665c5 ;
    foaf:name "Beatriz Esteves" .

_:N05cd1f43dbaf4b4ba297dab5ee221394 a dct:Agent,
        foaf:Person ;
    org:memberOf _:N2bfb2dfcc0b24c5182bd06c242c085fa ;
    foaf:homepage "https://www.linkedin.com/in/georg-philip-krog-a2a278104/" ;
    foaf:name "Georg P. Krog" .

_:N0a43dd9ea5e94fe695d8b7df8802cfdd a dct:Agent,
        foaf:Person ;
    scoro:hasORCID "0000-0002-5068-3714" ;
    org:memberOf _:N313d89a6c37147bfac1bbb4aa7f6510b ;
    foaf:homepage "https://harshp.com/" ;
    foaf:name "Harshvardhan J. Pandit" .

